<?xml version="1.0" encoding="ISO-8859-1"?>
<!DOCTYPE rdf:RDF [
	<!ENTITY java "http://localhost/~dennis/platformkit/2010_1/java.owl#">
	<!ENTITY j2se-5_0 "http://soft.vub.ac.be/platformkit/2010/1/j2se-5_0.owl#">
	<!ENTITY ns_33 "http://localhost/~dennis/platformkit/2010_1/">
	<!ENTITY android-1_6 "http://soft.vub.ac.be/platformkit/2010/1/android-1_6.owl#">
	<!ENTITY android-1_5 "http://soft.vub.ac.be/platformkit/2010/1/android-1_5.owl#">
	<!ENTITY isa "http://localhost/~dennis/platformkit/2010_1/isa.owl#">
	<!ENTITY platform "http://localhost/~dennis/platformkit/2010_1/platform.owl#">
	<!ENTITY xsd "http://www.w3.org/2001/XMLSchema#">
	<!ENTITY owl "http://www.w3.org/2002/07/owl#">
	<!ENTITY rdf "http://www.w3.org/1999/02/22-rdf-syntax-ns#">
	<!ENTITY rdfs "http://www.w3.org/2000/01/rdf-schema#">
]>
<rdf:RDF
	 xmlns:java="&java;"
	 xmlns:j2se-5_0="&j2se-5_0;"
	 xmlns:ns_33="&ns_33;"
	 xmlns:android-1_6="&android-1_6;"
	 xmlns:android-1_5="&android-1_5;"
	 xmlns:isa="&isa;"
	 xmlns:platform="&platform;"
	 xmlns:xsd="&xsd;"
	 xmlns:owl="&owl;"
	 xmlns:rdf="&rdf;"
	 xmlns:rdfs="&rdfs;"
>

	<owl:Ontology rdf:about="http://soft.vub.ac.be/platformkit/2010/1/android-1_6.owl#">
		<owl:versionInfo>$Id: UML2ToPackageAPIOntology.atl 8082 2010-03-18 21:11:00Z dwagelaa $</owl:versionInfo>
		<owl:imports rdf:resource="http://localhost/~dennis/platformkit/2010_1/platform.owl"/>
		<owl:imports rdf:resource="http://localhost/~dennis/platformkit/2010_1/java.owl"/>
		<owl:imports rdf:resource="http://soft.vub.ac.be/platformkit/2010/1/android-1_5.owl#"/>
		<owl:imports rdf:resource="http://localhost/~dennis/platformkit/2010_1/isa.owl"/>
		<owl:imports rdf:resource="http://soft.vub.ac.be/platformkit/2010/1/j2se-5_0.owl#"/>
		<rdfs:comment xml:lang="en">Generated by [UML2ToSimplifiedPackageAPIOntology.atl 8080 2010-03-18 10:46:40Z dwagelaa], [UML2ToPackageAPIOntology.atl 8082 2010-03-18 21:11:00Z dwagelaa], [UML2ToAPIOntology.atl 8086 2010-03-19 09:49:17Z dwagelaa], and [UML2Comparison.atl 8326 2010-11-11 13:32:14Z dwagelaa]</rdfs:comment>
		<rdfs:comment>Dennis Wagelaar &lt;dennis.wagelaar@vub.ac.be&gt;</rdfs:comment>
		<rdfs:comment xml:lang="en">&#169; 2010, Vrije Universiteit Brussel. All rights reserved.</rdfs:comment>
		<rdfs:label xml:lang="en">Android 1.6</rdfs:label>
	</owl:Ontology>
	<owl:Class rdf:about="&android-1_6;Android1_6API">
		<rdfs:subClassOf rdf:resource="&android-1_6;AndroidAPI"/>
		<rdfs:subClassOf rdf:resource="&android-1_6;AndroidAccessibilityserviceAPI"/>
		<rdfs:subClassOf rdf:resource="&android-1_6;AndroidAppAPI"/>
		<rdfs:subClassOf rdf:resource="&android-1_6;AndroidViewAPI"/>
		<rdfs:subClassOf rdf:resource="&android-1_6;AndroidViewAccessibilityAPI"/>
		<rdfs:subClassOf rdf:resource="&android-1_6;AndroidViewInputmethodAPI"/>
		<rdfs:subClassOf rdf:resource="&android-1_6;AndroidViewAnimationAPI"/>
		<rdfs:subClassOf rdf:resource="&android-1_6;AndroidContentAPI"/>
		<rdfs:subClassOf rdf:resource="&android-1_6;AndroidContentResAPI"/>
		<rdfs:subClassOf rdf:resource="&android-1_6;AndroidContentPmAPI"/>
		<rdfs:subClassOf rdf:resource="&android-1_6;AndroidOsAPI"/>
		<rdfs:subClassOf rdf:resource="&android-1_6;AndroidGraphicsAPI"/>
		<rdfs:subClassOf rdf:resource="&android-1_6;AndroidGraphicsDrawableAPI"/>
		<rdfs:subClassOf rdf:resource="&android-1_6;AndroidGraphicsDrawableShapesAPI"/>
		<rdfs:subClassOf rdf:resource="&android-1_6;AndroidNetAPI"/>
		<rdfs:subClassOf rdf:resource="&android-1_6;AndroidNetHttpAPI"/>
		<rdfs:subClassOf rdf:resource="&android-1_6;AndroidNetWifiAPI"/>
		<rdfs:subClassOf rdf:resource="&android-1_6;AndroidDatabaseAPI"/>
		<rdfs:subClassOf rdf:resource="&android-1_6;AndroidDatabaseSqliteAPI"/>
		<rdfs:subClassOf rdf:resource="&android-1_6;AndroidUtilAPI"/>
		<rdfs:subClassOf rdf:resource="&android-1_6;AndroidWidgetAPI"/>
		<rdfs:subClassOf rdf:resource="&android-1_6;AndroidAppwidgetAPI"/>
		<rdfs:subClassOf rdf:resource="&android-1_6;AndroidGestureAPI"/>
		<rdfs:subClassOf rdf:resource="&android-1_6;AndroidHardwareAPI"/>
		<rdfs:subClassOf rdf:resource="&android-1_6;AndroidInputmethodserviceAPI"/>
		<rdfs:subClassOf rdf:resource="&android-1_6;AndroidLocationAPI"/>
		<rdfs:subClassOf rdf:resource="&android-1_6;AndroidMediaAPI"/>
		<rdfs:subClassOf rdf:resource="&android-1_6;AndroidOpenglAPI"/>
		<rdfs:subClassOf rdf:resource="&android-1_6;AndroidPreferenceAPI"/>
		<rdfs:subClassOf rdf:resource="&android-1_6;AndroidProviderAPI"/>
		<rdfs:subClassOf rdf:resource="&android-1_6;AndroidWebkitAPI"/>
		<rdfs:subClassOf rdf:resource="&android-1_6;AndroidSaxAPI"/>
		<rdfs:subClassOf rdf:resource="&android-1_6;AndroidSpeechAPI"/>
		<rdfs:subClassOf rdf:resource="&android-1_6;AndroidSpeechTtsAPI"/>
		<rdfs:subClassOf rdf:resource="&android-1_6;AndroidTelephonyAPI"/>
		<rdfs:subClassOf rdf:resource="&android-1_6;AndroidTelephonyGsmAPI"/>
		<rdfs:subClassOf rdf:resource="&android-1_6;AndroidTextAPI"/>
		<rdfs:subClassOf rdf:resource="&android-1_6;AndroidTextFormatAPI"/>
		<rdfs:subClassOf rdf:resource="&android-1_6;AndroidTextMethodAPI"/>
		<rdfs:subClassOf rdf:resource="&android-1_6;AndroidTextStyleAPI"/>
		<rdfs:subClassOf rdf:resource="&android-1_6;AndroidTextUtilAPI"/>
		<rdfs:subClassOf rdf:resource="&android-1_6;AndroidTestAPI"/>
		<rdfs:subClassOf rdf:resource="&android-1_6;AndroidTestMockAPI"/>
		<rdfs:subClassOf rdf:resource="&android-1_6;AndroidTestSuitebuilderAPI"/>
		<rdfs:subClassOf rdf:resource="&android-1_6;AndroidTestSuitebuilderAnnotationAPI"/>
		<rdfs:subClassOf rdf:resource="&android-1_6;JavaLangAPI"/>
		<rdfs:subClassOf rdf:resource="&android-1_6;JavaLangAnnotationAPI"/>
		<rdfs:subClassOf rdf:resource="&android-1_6;JavaLangReflectAPI"/>
		<rdfs:subClassOf rdf:resource="&android-1_6;JavaLangRefAPI"/>
		<rdfs:subClassOf rdf:resource="&android-1_6;JavaUtilAPI"/>
		<rdfs:subClassOf rdf:resource="&android-1_6;JavaUtilConcurrentAPI"/>
		<rdfs:subClassOf rdf:resource="&android-1_6;JavaUtilConcurrentAtomicAPI"/>
		<rdfs:subClassOf rdf:resource="&android-1_6;JavaUtilConcurrentLocksAPI"/>
		<rdfs:subClassOf rdf:resource="&android-1_6;JavaUtilRegexAPI"/>
		<rdfs:subClassOf rdf:resource="&android-1_6;JavaUtilJarAPI"/>
		<rdfs:subClassOf rdf:resource="&android-1_6;JavaUtilZipAPI"/>
		<rdfs:subClassOf rdf:resource="&android-1_6;JavaUtilLoggingAPI"/>
		<rdfs:subClassOf rdf:resource="&android-1_6;JavaUtilPrefsAPI"/>
		<rdfs:subClassOf rdf:resource="&android-1_6;JavaIoAPI"/>
		<rdfs:subClassOf rdf:resource="&android-1_6;JavaNioAPI"/>
		<rdfs:subClassOf rdf:resource="&android-1_6;JavaNioChannelsAPI"/>
		<rdfs:subClassOf rdf:resource="&android-1_6;JavaNioChannelsSpiAPI"/>
		<rdfs:subClassOf rdf:resource="&android-1_6;JavaNioCharsetAPI"/>
		<rdfs:subClassOf rdf:resource="&android-1_6;JavaNioCharsetSpiAPI"/>
		<rdfs:subClassOf rdf:resource="&android-1_6;JavaNetAPI"/>
		<rdfs:subClassOf rdf:resource="&android-1_6;JavaSecurityAPI"/>
		<rdfs:subClassOf rdf:resource="&android-1_6;JavaSecurityCertAPI"/>
		<rdfs:subClassOf rdf:resource="&android-1_6;JavaSecuritySpecAPI"/>
		<rdfs:subClassOf rdf:resource="&android-1_6;JavaSecurityAclAPI"/>
		<rdfs:subClassOf rdf:resource="&android-1_6;JavaSecurityInterfacesAPI"/>
		<rdfs:subClassOf rdf:resource="&android-1_6;JavaTextAPI"/>
		<rdfs:subClassOf rdf:resource="&android-1_6;JavaAwtFontAPI"/>
		<rdfs:subClassOf rdf:resource="&android-1_6;JavaBeansAPI"/>
		<rdfs:subClassOf rdf:resource="&android-1_6;JavaMathAPI"/>
		<rdfs:subClassOf rdf:resource="&android-1_6;JavaSqlAPI"/>
		<rdfs:subClassOf rdf:resource="&android-1_6;OrgXmlpullV1API"/>
		<rdfs:subClassOf rdf:resource="&android-1_6;OrgXmlpullV1Sax2API"/>
		<rdfs:subClassOf rdf:resource="&android-1_6;OrgXmlSaxAPI"/>
		<rdfs:subClassOf rdf:resource="&android-1_6;OrgXmlSaxHelpersAPI"/>
		<rdfs:subClassOf rdf:resource="&android-1_6;OrgXmlSaxExtAPI"/>
		<rdfs:subClassOf rdf:resource="&android-1_6;OrgW3cDomAPI"/>
		<rdfs:subClassOf rdf:resource="&android-1_6;OrgApacheCommonsLoggingAPI"/>
		<rdfs:subClassOf rdf:resource="&android-1_6;OrgApacheHttpAPI"/>
		<rdfs:subClassOf rdf:resource="&android-1_6;OrgApacheHttpProtocolAPI"/>
		<rdfs:subClassOf rdf:resource="&android-1_6;OrgApacheHttpUtilAPI"/>
		<rdfs:subClassOf rdf:resource="&android-1_6;OrgApacheHttpParamsAPI"/>
		<rdfs:subClassOf rdf:resource="&android-1_6;OrgApacheHttpAuthAPI"/>
		<rdfs:subClassOf rdf:resource="&android-1_6;OrgApacheHttpAuthParamsAPI"/>
		<rdfs:subClassOf rdf:resource="&android-1_6;OrgApacheHttpClientAPI"/>
		<rdfs:subClassOf rdf:resource="&android-1_6;OrgApacheHttpClientMethodsAPI"/>
		<rdfs:subClassOf rdf:resource="&android-1_6;OrgApacheHttpClientEntityAPI"/>
		<rdfs:subClassOf rdf:resource="&android-1_6;OrgApacheHttpClientParamsAPI"/>
		<rdfs:subClassOf rdf:resource="&android-1_6;OrgApacheHttpClientProtocolAPI"/>
		<rdfs:subClassOf rdf:resource="&android-1_6;OrgApacheHttpClientUtilsAPI"/>
		<rdfs:subClassOf rdf:resource="&android-1_6;OrgApacheHttpCookieAPI"/>
		<rdfs:subClassOf rdf:resource="&android-1_6;OrgApacheHttpCookieParamsAPI"/>
		<rdfs:subClassOf rdf:resource="&android-1_6;OrgApacheHttpConnAPI"/>
		<rdfs:subClassOf rdf:resource="&android-1_6;OrgApacheHttpConnParamsAPI"/>
		<rdfs:subClassOf rdf:resource="&android-1_6;OrgApacheHttpConnSchemeAPI"/>
		<rdfs:subClassOf rdf:resource="&android-1_6;OrgApacheHttpConnRoutingAPI"/>
		<rdfs:subClassOf rdf:resource="&android-1_6;OrgApacheHttpConnSslAPI"/>
		<rdfs:subClassOf rdf:resource="&android-1_6;OrgApacheHttpConnUtilAPI"/>
		<rdfs:subClassOf rdf:resource="&android-1_6;OrgApacheHttpEntityAPI"/>
		<rdfs:subClassOf rdf:resource="&android-1_6;OrgApacheHttpMessageAPI"/>
		<rdfs:subClassOf rdf:resource="&android-1_6;OrgApacheHttpImplAPI"/>
		<rdfs:subClassOf rdf:resource="&android-1_6;OrgApacheHttpImplEntityAPI"/>
		<rdfs:subClassOf rdf:resource="&android-1_6;OrgApacheHttpImplAuthAPI"/>
		<rdfs:subClassOf rdf:resource="&android-1_6;OrgApacheHttpImplClientAPI"/>
		<rdfs:subClassOf rdf:resource="&android-1_6;OrgApacheHttpImplConnAPI"/>
		<rdfs:subClassOf rdf:resource="&android-1_6;OrgApacheHttpImplConnTsccmAPI"/>
		<rdfs:subClassOf rdf:resource="&android-1_6;OrgApacheHttpImplIoAPI"/>
		<rdfs:subClassOf rdf:resource="&android-1_6;OrgApacheHttpImplCookieAPI"/>
		<rdfs:subClassOf rdf:resource="&android-1_6;OrgApacheHttpIoAPI"/>
		<rdfs:subClassOf rdf:resource="&android-1_6;OrgJsonAPI"/>
		<rdfs:subClassOf rdf:resource="&android-1_6;JavaxMicroeditionKhronosOpenglesAPI"/>
		<rdfs:subClassOf rdf:resource="&android-1_6;JavaxMicroeditionKhronosEglAPI"/>
		<rdfs:subClassOf rdf:resource="&android-1_6;JavaxNetAPI"/>
		<rdfs:subClassOf rdf:resource="&android-1_6;JavaxNetSslAPI"/>
		<rdfs:subClassOf rdf:resource="&android-1_6;JavaxSecurityAuthAPI"/>
		<rdfs:subClassOf rdf:resource="&android-1_6;JavaxSecurityAuthCallbackAPI"/>
		<rdfs:subClassOf rdf:resource="&android-1_6;JavaxSecurityAuthX500API"/>
		<rdfs:subClassOf rdf:resource="&android-1_6;JavaxSecurityAuthLoginAPI"/>
		<rdfs:subClassOf rdf:resource="&android-1_6;JavaxSecurityCertAPI"/>
		<rdfs:subClassOf rdf:resource="&android-1_6;JavaxCryptoAPI"/>
		<rdfs:subClassOf rdf:resource="&android-1_6;JavaxCryptoInterfacesAPI"/>
		<rdfs:subClassOf rdf:resource="&android-1_6;JavaxCryptoSpecAPI"/>
		<rdfs:subClassOf rdf:resource="&android-1_6;JavaxSqlAPI"/>
		<rdfs:subClassOf rdf:resource="&android-1_6;JavaxXmlAPI"/>
		<rdfs:subClassOf rdf:resource="&android-1_6;JavaxXmlParsersAPI"/>
		<rdfs:subClassOf rdf:resource="&android-1_6;JunitFrameworkAPI"/>
		<rdfs:subClassOf rdf:resource="&android-1_6;JunitRunnerAPI"/>
		<rdfs:subClassOf rdf:resource="&android-1_6;DalvikAnnotationAPI"/>
		<rdfs:subClassOf rdf:resource="&android-1_6;DalvikBytecodeAPI"/>
		<rdfs:subClassOf rdf:resource="&android-1_6;DalvikSystemAPI"/>
		<rdfs:comment xml:lang="en">Android 1.6 API</rdfs:comment>
		<rdfs:comment xml:lang="OWLManchester">platform:comprisesInterfacePart some Android and platform:comprisesInterfacePart some AndroidAccessibilityservice and platform:comprisesInterfacePart some AndroidApp and platform:comprisesInterfacePart some AndroidView and platform:comprisesInterfacePart some AndroidViewAccessibility and platform:comprisesInterfacePart some AndroidViewInputmethod and platform:comprisesInterfacePart some AndroidViewAnimation and platform:comprisesInterfacePart some AndroidContent and platform:comprisesInterfacePart some AndroidContentRes and platform:comprisesInterfacePart some AndroidContentPm and platform:comprisesInterfacePart some AndroidOs and platform:comprisesInterfacePart some AndroidGraphics and platform:comprisesInterfacePart some AndroidGraphicsDrawable and platform:comprisesInterfacePart some AndroidGraphicsDrawableShapes and platform:comprisesInterfacePart some AndroidNet and platform:comprisesInterfacePart some AndroidNetHttp and platform:comprisesInterfacePart some AndroidNetWifi and platform:comprisesInterfacePart some AndroidDatabase and platform:comprisesInterfacePart some AndroidDatabaseSqlite and platform:comprisesInterfacePart some AndroidUtil and platform:comprisesInterfacePart some AndroidWidget and platform:comprisesInterfacePart some AndroidAppwidget and platform:comprisesInterfacePart some AndroidGesture and platform:comprisesInterfacePart some AndroidHardware and platform:comprisesInterfacePart some AndroidInputmethodservice and platform:comprisesInterfacePart some AndroidLocation and platform:comprisesInterfacePart some AndroidMedia and platform:comprisesInterfacePart some AndroidOpengl and platform:comprisesInterfacePart some AndroidPreference and platform:comprisesInterfacePart some AndroidProvider and platform:comprisesInterfacePart some AndroidWebkit and platform:comprisesInterfacePart some AndroidSax and platform:comprisesInterfacePart some AndroidSpeech and platform:comprisesInterfacePart some AndroidSpeechTts and platform:comprisesInterfacePart some AndroidTelephony and platform:comprisesInterfacePart some AndroidTelephonyGsm and platform:comprisesInterfacePart some AndroidText and platform:comprisesInterfacePart some AndroidTextFormat and platform:comprisesInterfacePart some AndroidTextMethod and platform:comprisesInterfacePart some AndroidTextStyle and platform:comprisesInterfacePart some AndroidTextUtil and platform:comprisesInterfacePart some AndroidTest and platform:comprisesInterfacePart some AndroidTestMock and platform:comprisesInterfacePart some AndroidTestSuitebuilder and platform:comprisesInterfacePart some AndroidTestSuitebuilderAnnotation and platform:comprisesInterfacePart some JavaLang and platform:comprisesInterfacePart some JavaLangAnnotation and platform:comprisesInterfacePart some JavaLangReflect and platform:comprisesInterfacePart some JavaLangRef and platform:comprisesInterfacePart some JavaUtil and platform:comprisesInterfacePart some JavaUtilConcurrent and platform:comprisesInterfacePart some JavaUtilConcurrentAtomic and platform:comprisesInterfacePart some JavaUtilConcurrentLocks and platform:comprisesInterfacePart some JavaUtilRegex and platform:comprisesInterfacePart some JavaUtilJar and platform:comprisesInterfacePart some JavaUtilZip and platform:comprisesInterfacePart some JavaUtilLogging and platform:comprisesInterfacePart some JavaUtilPrefs and platform:comprisesInterfacePart some JavaIo and platform:comprisesInterfacePart some JavaNio and platform:comprisesInterfacePart some JavaNioChannels and platform:comprisesInterfacePart some JavaNioChannelsSpi and platform:comprisesInterfacePart some JavaNioCharset and platform:comprisesInterfacePart some JavaNioCharsetSpi and platform:comprisesInterfacePart some JavaNet and platform:comprisesInterfacePart some JavaSecurity and platform:comprisesInterfacePart some JavaSecurityCert and platform:comprisesInterfacePart some JavaSecuritySpec and platform:comprisesInterfacePart some JavaSecurityAcl and platform:comprisesInterfacePart some JavaSecurityInterfaces and platform:comprisesInterfacePart some JavaText and platform:comprisesInterfacePart some JavaAwtFont and platform:comprisesInterfacePart some JavaBeans and platform:comprisesInterfacePart some JavaMath and platform:comprisesInterfacePart some JavaSql and platform:comprisesInterfacePart some OrgXmlpullV1 and platform:comprisesInterfacePart some OrgXmlpullV1Sax2 and platform:comprisesInterfacePart some OrgXmlSax and platform:comprisesInterfacePart some OrgXmlSaxHelpers and platform:comprisesInterfacePart some OrgXmlSaxExt and platform:comprisesInterfacePart some OrgW3cDom and platform:comprisesInterfacePart some OrgApacheCommonsLogging and platform:comprisesInterfacePart some OrgApacheHttp and platform:comprisesInterfacePart some OrgApacheHttpProtocol and platform:comprisesInterfacePart some OrgApacheHttpUtil and platform:comprisesInterfacePart some OrgApacheHttpParams and platform:comprisesInterfacePart some OrgApacheHttpAuth and platform:comprisesInterfacePart some OrgApacheHttpAuthParams and platform:comprisesInterfacePart some OrgApacheHttpClient and platform:comprisesInterfacePart some OrgApacheHttpClientMethods and platform:comprisesInterfacePart some OrgApacheHttpClientEntity and platform:comprisesInterfacePart some OrgApacheHttpClientParams and platform:comprisesInterfacePart some OrgApacheHttpClientProtocol and platform:comprisesInterfacePart some OrgApacheHttpClientUtils and platform:comprisesInterfacePart some OrgApacheHttpCookie and platform:comprisesInterfacePart some OrgApacheHttpCookieParams and platform:comprisesInterfacePart some OrgApacheHttpConn and platform:comprisesInterfacePart some OrgApacheHttpConnParams and platform:comprisesInterfacePart some OrgApacheHttpConnScheme and platform:comprisesInterfacePart some OrgApacheHttpConnRouting and platform:comprisesInterfacePart some OrgApacheHttpConnSsl and platform:comprisesInterfacePart some OrgApacheHttpConnUtil and platform:comprisesInterfacePart some OrgApacheHttpEntity and platform:comprisesInterfacePart some OrgApacheHttpMessage and platform:comprisesInterfacePart some OrgApacheHttpImpl and platform:comprisesInterfacePart some OrgApacheHttpImplEntity and platform:comprisesInterfacePart some OrgApacheHttpImplAuth and platform:comprisesInterfacePart some OrgApacheHttpImplClient and platform:comprisesInterfacePart some OrgApacheHttpImplConn and platform:comprisesInterfacePart some OrgApacheHttpImplConnTsccm and platform:comprisesInterfacePart some OrgApacheHttpImplIo and platform:comprisesInterfacePart some OrgApacheHttpImplCookie and platform:comprisesInterfacePart some OrgApacheHttpIo and platform:comprisesInterfacePart some OrgJson and platform:comprisesInterfacePart some JavaxMicroeditionKhronosOpengles and platform:comprisesInterfacePart some JavaxMicroeditionKhronosEgl and platform:comprisesInterfacePart some JavaxNet and platform:comprisesInterfacePart some JavaxNetSsl and platform:comprisesInterfacePart some JavaxSecurityAuth and platform:comprisesInterfacePart some JavaxSecurityAuthCallback and platform:comprisesInterfacePart some JavaxSecurityAuthX500 and platform:comprisesInterfacePart some JavaxSecurityAuthLogin and platform:comprisesInterfacePart some JavaxSecurityCert and platform:comprisesInterfacePart some JavaxCrypto and platform:comprisesInterfacePart some JavaxCryptoInterfaces and platform:comprisesInterfacePart some JavaxCryptoSpec and platform:comprisesInterfacePart some JavaxSql and platform:comprisesInterfacePart some JavaxXml and platform:comprisesInterfacePart some JavaxXmlParsers and platform:comprisesInterfacePart some JunitFramework and platform:comprisesInterfacePart some JunitRunner and platform:comprisesInterfacePart some DalvikAnnotation and platform:comprisesInterfacePart some DalvikBytecode and platform:comprisesInterfacePart some DalvikSystem</rdfs:comment>
	</owl:Class>
	<owl:Class rdf:about="&android-1_6;Android1_6ClassLibrary">
		<rdfs:subClassOf rdf:resource="&android-1_6;AndroidClassLibrary"/>
		<rdfs:subClassOf rdf:resource="&android-1_6;AndroidAccessibilityserviceClassLibrary"/>
		<rdfs:subClassOf rdf:resource="&android-1_6;AndroidAppClassLibrary"/>
		<rdfs:subClassOf rdf:resource="&android-1_6;AndroidViewClassLibrary"/>
		<rdfs:subClassOf rdf:resource="&android-1_6;AndroidViewAccessibilityClassLibrary"/>
		<rdfs:subClassOf rdf:resource="&android-1_6;AndroidViewInputmethodClassLibrary"/>
		<rdfs:subClassOf rdf:resource="&android-1_6;AndroidViewAnimationClassLibrary"/>
		<rdfs:subClassOf rdf:resource="&android-1_6;AndroidContentClassLibrary"/>
		<rdfs:subClassOf rdf:resource="&android-1_6;AndroidContentResClassLibrary"/>
		<rdfs:subClassOf rdf:resource="&android-1_6;AndroidContentPmClassLibrary"/>
		<rdfs:subClassOf rdf:resource="&android-1_6;AndroidOsClassLibrary"/>
		<rdfs:subClassOf rdf:resource="&android-1_6;AndroidGraphicsClassLibrary"/>
		<rdfs:subClassOf rdf:resource="&android-1_6;AndroidGraphicsDrawableClassLibrary"/>
		<rdfs:subClassOf rdf:resource="&android-1_6;AndroidGraphicsDrawableShapesClassLibrary"/>
		<rdfs:subClassOf rdf:resource="&android-1_6;AndroidNetClassLibrary"/>
		<rdfs:subClassOf rdf:resource="&android-1_6;AndroidNetHttpClassLibrary"/>
		<rdfs:subClassOf rdf:resource="&android-1_6;AndroidNetWifiClassLibrary"/>
		<rdfs:subClassOf rdf:resource="&android-1_6;AndroidDatabaseClassLibrary"/>
		<rdfs:subClassOf rdf:resource="&android-1_6;AndroidDatabaseSqliteClassLibrary"/>
		<rdfs:subClassOf rdf:resource="&android-1_6;AndroidUtilClassLibrary"/>
		<rdfs:subClassOf rdf:resource="&android-1_6;AndroidWidgetClassLibrary"/>
		<rdfs:subClassOf rdf:resource="&android-1_6;AndroidAppwidgetClassLibrary"/>
		<rdfs:subClassOf rdf:resource="&android-1_6;AndroidGestureClassLibrary"/>
		<rdfs:subClassOf rdf:resource="&android-1_6;AndroidHardwareClassLibrary"/>
		<rdfs:subClassOf rdf:resource="&android-1_6;AndroidInputmethodserviceClassLibrary"/>
		<rdfs:subClassOf rdf:resource="&android-1_6;AndroidLocationClassLibrary"/>
		<rdfs:subClassOf rdf:resource="&android-1_6;AndroidMediaClassLibrary"/>
		<rdfs:subClassOf rdf:resource="&android-1_6;AndroidOpenglClassLibrary"/>
		<rdfs:subClassOf rdf:resource="&android-1_6;AndroidPreferenceClassLibrary"/>
		<rdfs:subClassOf rdf:resource="&android-1_6;AndroidProviderClassLibrary"/>
		<rdfs:subClassOf rdf:resource="&android-1_6;AndroidWebkitClassLibrary"/>
		<rdfs:subClassOf rdf:resource="&android-1_6;AndroidSaxClassLibrary"/>
		<rdfs:subClassOf rdf:resource="&android-1_6;AndroidSpeechClassLibrary"/>
		<rdfs:subClassOf rdf:resource="&android-1_6;AndroidSpeechTtsClassLibrary"/>
		<rdfs:subClassOf rdf:resource="&android-1_6;AndroidTelephonyClassLibrary"/>
		<rdfs:subClassOf rdf:resource="&android-1_6;AndroidTelephonyGsmClassLibrary"/>
		<rdfs:subClassOf rdf:resource="&android-1_6;AndroidTextClassLibrary"/>
		<rdfs:subClassOf rdf:resource="&android-1_6;AndroidTextFormatClassLibrary"/>
		<rdfs:subClassOf rdf:resource="&android-1_6;AndroidTextMethodClassLibrary"/>
		<rdfs:subClassOf rdf:resource="&android-1_6;AndroidTextStyleClassLibrary"/>
		<rdfs:subClassOf rdf:resource="&android-1_6;AndroidTextUtilClassLibrary"/>
		<rdfs:subClassOf rdf:resource="&android-1_6;AndroidTestClassLibrary"/>
		<rdfs:subClassOf rdf:resource="&android-1_6;AndroidTestMockClassLibrary"/>
		<rdfs:subClassOf rdf:resource="&android-1_6;AndroidTestSuitebuilderClassLibrary"/>
		<rdfs:subClassOf rdf:resource="&android-1_6;AndroidTestSuitebuilderAnnotationClassLibrary"/>
		<rdfs:subClassOf rdf:resource="&android-1_6;JavaLangClassLibrary"/>
		<rdfs:subClassOf rdf:resource="&android-1_6;JavaLangAnnotationClassLibrary"/>
		<rdfs:subClassOf rdf:resource="&android-1_6;JavaLangReflectClassLibrary"/>
		<rdfs:subClassOf rdf:resource="&android-1_6;JavaLangRefClassLibrary"/>
		<rdfs:subClassOf rdf:resource="&android-1_6;JavaUtilClassLibrary"/>
		<rdfs:subClassOf rdf:resource="&android-1_6;JavaUtilConcurrentClassLibrary"/>
		<rdfs:subClassOf rdf:resource="&android-1_6;JavaUtilConcurrentAtomicClassLibrary"/>
		<rdfs:subClassOf rdf:resource="&android-1_6;JavaUtilConcurrentLocksClassLibrary"/>
		<rdfs:subClassOf rdf:resource="&android-1_6;JavaUtilRegexClassLibrary"/>
		<rdfs:subClassOf rdf:resource="&android-1_6;JavaUtilJarClassLibrary"/>
		<rdfs:subClassOf rdf:resource="&android-1_6;JavaUtilZipClassLibrary"/>
		<rdfs:subClassOf rdf:resource="&android-1_6;JavaUtilLoggingClassLibrary"/>
		<rdfs:subClassOf rdf:resource="&android-1_6;JavaUtilPrefsClassLibrary"/>
		<rdfs:subClassOf rdf:resource="&android-1_6;JavaIoClassLibrary"/>
		<rdfs:subClassOf rdf:resource="&android-1_6;JavaNioClassLibrary"/>
		<rdfs:subClassOf rdf:resource="&android-1_6;JavaNioChannelsClassLibrary"/>
		<rdfs:subClassOf rdf:resource="&android-1_6;JavaNioChannelsSpiClassLibrary"/>
		<rdfs:subClassOf rdf:resource="&android-1_6;JavaNioCharsetClassLibrary"/>
		<rdfs:subClassOf rdf:resource="&android-1_6;JavaNioCharsetSpiClassLibrary"/>
		<rdfs:subClassOf rdf:resource="&android-1_6;JavaNetClassLibrary"/>
		<rdfs:subClassOf rdf:resource="&android-1_6;JavaSecurityClassLibrary"/>
		<rdfs:subClassOf rdf:resource="&android-1_6;JavaSecurityCertClassLibrary"/>
		<rdfs:subClassOf rdf:resource="&android-1_6;JavaSecuritySpecClassLibrary"/>
		<rdfs:subClassOf rdf:resource="&android-1_6;JavaSecurityAclClassLibrary"/>
		<rdfs:subClassOf rdf:resource="&android-1_6;JavaSecurityInterfacesClassLibrary"/>
		<rdfs:subClassOf rdf:resource="&android-1_6;JavaTextClassLibrary"/>
		<rdfs:subClassOf rdf:resource="&android-1_6;JavaAwtFontClassLibrary"/>
		<rdfs:subClassOf rdf:resource="&android-1_6;JavaBeansClassLibrary"/>
		<rdfs:subClassOf rdf:resource="&android-1_6;JavaMathClassLibrary"/>
		<rdfs:subClassOf rdf:resource="&android-1_6;JavaSqlClassLibrary"/>
		<rdfs:subClassOf rdf:resource="&android-1_6;OrgXmlpullV1ClassLibrary"/>
		<rdfs:subClassOf rdf:resource="&android-1_6;OrgXmlpullV1Sax2ClassLibrary"/>
		<rdfs:subClassOf rdf:resource="&android-1_6;OrgXmlSaxClassLibrary"/>
		<rdfs:subClassOf rdf:resource="&android-1_6;OrgXmlSaxHelpersClassLibrary"/>
		<rdfs:subClassOf rdf:resource="&android-1_6;OrgXmlSaxExtClassLibrary"/>
		<rdfs:subClassOf rdf:resource="&android-1_6;OrgW3cDomClassLibrary"/>
		<rdfs:subClassOf rdf:resource="&android-1_6;OrgApacheCommonsLoggingClassLibrary"/>
		<rdfs:subClassOf rdf:resource="&android-1_6;OrgApacheHttpClassLibrary"/>
		<rdfs:subClassOf rdf:resource="&android-1_6;OrgApacheHttpProtocolClassLibrary"/>
		<rdfs:subClassOf rdf:resource="&android-1_6;OrgApacheHttpUtilClassLibrary"/>
		<rdfs:subClassOf rdf:resource="&android-1_6;OrgApacheHttpParamsClassLibrary"/>
		<rdfs:subClassOf rdf:resource="&android-1_6;OrgApacheHttpAuthClassLibrary"/>
		<rdfs:subClassOf rdf:resource="&android-1_6;OrgApacheHttpAuthParamsClassLibrary"/>
		<rdfs:subClassOf rdf:resource="&android-1_6;OrgApacheHttpClientClassLibrary"/>
		<rdfs:subClassOf rdf:resource="&android-1_6;OrgApacheHttpClientMethodsClassLibrary"/>
		<rdfs:subClassOf rdf:resource="&android-1_6;OrgApacheHttpClientEntityClassLibrary"/>
		<rdfs:subClassOf rdf:resource="&android-1_6;OrgApacheHttpClientParamsClassLibrary"/>
		<rdfs:subClassOf rdf:resource="&android-1_6;OrgApacheHttpClientProtocolClassLibrary"/>
		<rdfs:subClassOf rdf:resource="&android-1_6;OrgApacheHttpClientUtilsClassLibrary"/>
		<rdfs:subClassOf rdf:resource="&android-1_6;OrgApacheHttpCookieClassLibrary"/>
		<rdfs:subClassOf rdf:resource="&android-1_6;OrgApacheHttpCookieParamsClassLibrary"/>
		<rdfs:subClassOf rdf:resource="&android-1_6;OrgApacheHttpConnClassLibrary"/>
		<rdfs:subClassOf rdf:resource="&android-1_6;OrgApacheHttpConnParamsClassLibrary"/>
		<rdfs:subClassOf rdf:resource="&android-1_6;OrgApacheHttpConnSchemeClassLibrary"/>
		<rdfs:subClassOf rdf:resource="&android-1_6;OrgApacheHttpConnRoutingClassLibrary"/>
		<rdfs:subClassOf rdf:resource="&android-1_6;OrgApacheHttpConnSslClassLibrary"/>
		<rdfs:subClassOf rdf:resource="&android-1_6;OrgApacheHttpConnUtilClassLibrary"/>
		<rdfs:subClassOf rdf:resource="&android-1_6;OrgApacheHttpEntityClassLibrary"/>
		<rdfs:subClassOf rdf:resource="&android-1_6;OrgApacheHttpMessageClassLibrary"/>
		<rdfs:subClassOf rdf:resource="&android-1_6;OrgApacheHttpImplClassLibrary"/>
		<rdfs:subClassOf rdf:resource="&android-1_6;OrgApacheHttpImplEntityClassLibrary"/>
		<rdfs:subClassOf rdf:resource="&android-1_6;OrgApacheHttpImplAuthClassLibrary"/>
		<rdfs:subClassOf rdf:resource="&android-1_6;OrgApacheHttpImplClientClassLibrary"/>
		<rdfs:subClassOf rdf:resource="&android-1_6;OrgApacheHttpImplConnClassLibrary"/>
		<rdfs:subClassOf rdf:resource="&android-1_6;OrgApacheHttpImplConnTsccmClassLibrary"/>
		<rdfs:subClassOf rdf:resource="&android-1_6;OrgApacheHttpImplIoClassLibrary"/>
		<rdfs:subClassOf rdf:resource="&android-1_6;OrgApacheHttpImplCookieClassLibrary"/>
		<rdfs:subClassOf rdf:resource="&android-1_6;OrgApacheHttpIoClassLibrary"/>
		<rdfs:subClassOf rdf:resource="&android-1_6;OrgJsonClassLibrary"/>
		<rdfs:subClassOf rdf:resource="&android-1_6;JavaxMicroeditionKhronosOpenglesClassLibrary"/>
		<rdfs:subClassOf rdf:resource="&android-1_6;JavaxMicroeditionKhronosEglClassLibrary"/>
		<rdfs:subClassOf rdf:resource="&android-1_6;JavaxNetClassLibrary"/>
		<rdfs:subClassOf rdf:resource="&android-1_6;JavaxNetSslClassLibrary"/>
		<rdfs:subClassOf rdf:resource="&android-1_6;JavaxSecurityAuthClassLibrary"/>
		<rdfs:subClassOf rdf:resource="&android-1_6;JavaxSecurityAuthCallbackClassLibrary"/>
		<rdfs:subClassOf rdf:resource="&android-1_6;JavaxSecurityAuthX500ClassLibrary"/>
		<rdfs:subClassOf rdf:resource="&android-1_6;JavaxSecurityAuthLoginClassLibrary"/>
		<rdfs:subClassOf rdf:resource="&android-1_6;JavaxSecurityCertClassLibrary"/>
		<rdfs:subClassOf rdf:resource="&android-1_6;JavaxCryptoClassLibrary"/>
		<rdfs:subClassOf rdf:resource="&android-1_6;JavaxCryptoInterfacesClassLibrary"/>
		<rdfs:subClassOf rdf:resource="&android-1_6;JavaxCryptoSpecClassLibrary"/>
		<rdfs:subClassOf rdf:resource="&android-1_6;JavaxSqlClassLibrary"/>
		<rdfs:subClassOf rdf:resource="&android-1_6;JavaxXmlClassLibrary"/>
		<rdfs:subClassOf rdf:resource="&android-1_6;JavaxXmlParsersClassLibrary"/>
		<rdfs:subClassOf rdf:resource="&android-1_6;JunitFrameworkClassLibrary"/>
		<rdfs:subClassOf rdf:resource="&android-1_6;JunitRunnerClassLibrary"/>
		<rdfs:subClassOf rdf:resource="&android-1_6;DalvikAnnotationClassLibrary"/>
		<rdfs:subClassOf rdf:resource="&android-1_6;DalvikBytecodeClassLibrary"/>
		<rdfs:subClassOf rdf:resource="&android-1_6;DalvikSystemClassLibrary"/>
		<rdfs:comment xml:lang="en">Java class library implementing the Android 1.6 API</rdfs:comment>
		<rdfs:comment xml:lang="OWLManchester">platform:implementsInterface some Android1_6API</rdfs:comment>
	</owl:Class>
	<owl:Class rdf:about="&android-1_6;Android1_6BytecodeFormat">
		<owl:equivalentClass rdf:resource="&j2se-5_0;J2SE5_0BytecodeFormat"/>
		<owl:equivalentClass rdf:resource="&android-1_5;Android1_5BytecodeFormat"/>
		<rdfs:subClassOf rdf:resource="&isa;JavaBytecode"/>
		<rdfs:comment xml:lang="en">Android 1.6 bytecode format</rdfs:comment>
		<rdfs:comment xml:lang="OWLManchester">java:majorVersionNumber some xsd:integer[>="49"^^xsd:integer] and java:preverified value false</rdfs:comment>
	</owl:Class>
	<android-1_6:Android1_6BytecodeFormat rdf:about="&android-1_6;theAndroid1_6BytecodeFormat">
		<java:preverified rdf:datatype="http://www.w3.org/2001/XMLSchema#boolean">false</java:preverified>
		<java:minorVersionNumber rdf:datatype="http://www.w3.org/2001/XMLSchema#integer">0</java:minorVersionNumber>
		<java:majorVersionNumber rdf:datatype="http://www.w3.org/2001/XMLSchema#integer">49</java:majorVersionNumber>
	</android-1_6:Android1_6BytecodeFormat>
	<android-1_6:Android1_6API rdf:about="&android-1_6;theAndroid1_6API">
		<platform:comprisesInterfacePart rdf:resource="&android-1_6;theDalvikSystemPart"/>
		<platform:comprisesInterfacePart rdf:resource="&android-1_6;theDalvikBytecodePart"/>
		<platform:comprisesInterfacePart rdf:resource="&android-1_6;theDalvikAnnotationPart"/>
		<platform:comprisesInterfacePart rdf:resource="&android-1_6;theJunitRunnerPart"/>
		<platform:comprisesInterfacePart rdf:resource="&android-1_6;theJunitFrameworkPart"/>
		<platform:comprisesInterfacePart rdf:resource="&android-1_6;theJavaxXmlParsersPart"/>
		<platform:comprisesInterfacePart rdf:resource="&android-1_6;theJavaxXmlPart"/>
		<platform:comprisesInterfacePart rdf:resource="&android-1_6;theJavaxSqlPart"/>
		<platform:comprisesInterfacePart rdf:resource="&android-1_6;theJavaxCryptoSpecPart"/>
		<platform:comprisesInterfacePart rdf:resource="&android-1_6;theJavaxCryptoInterfacesPart"/>
		<platform:comprisesInterfacePart rdf:resource="&android-1_6;theJavaxCryptoPart"/>
		<platform:comprisesInterfacePart rdf:resource="&android-1_6;theJavaxSecurityCertPart"/>
		<platform:comprisesInterfacePart rdf:resource="&android-1_6;theJavaxSecurityAuthLoginPart"/>
		<platform:comprisesInterfacePart rdf:resource="&android-1_6;theJavaxSecurityAuthX500Part"/>
		<platform:comprisesInterfacePart rdf:resource="&android-1_6;theJavaxSecurityAuthCallbackPart"/>
		<platform:comprisesInterfacePart rdf:resource="&android-1_6;theJavaxSecurityAuthPart"/>
		<platform:comprisesInterfacePart rdf:resource="&android-1_6;theJavaxNetSslPart"/>
		<platform:comprisesInterfacePart rdf:resource="&android-1_6;theJavaxNetPart"/>
		<platform:comprisesInterfacePart rdf:resource="&android-1_6;theJavaxMicroeditionKhronosEglPart"/>
		<platform:comprisesInterfacePart rdf:resource="&android-1_6;theJavaxMicroeditionKhronosOpenglesPart"/>
		<platform:comprisesInterfacePart rdf:resource="&android-1_6;theOrgJsonPart"/>
		<platform:comprisesInterfacePart rdf:resource="&android-1_6;theOrgApacheHttpIoPart"/>
		<platform:comprisesInterfacePart rdf:resource="&android-1_6;theOrgApacheHttpImplCookiePart"/>
		<platform:comprisesInterfacePart rdf:resource="&android-1_6;theOrgApacheHttpImplIoPart"/>
		<platform:comprisesInterfacePart rdf:resource="&android-1_6;theOrgApacheHttpImplConnTsccmPart"/>
		<platform:comprisesInterfacePart rdf:resource="&android-1_6;theOrgApacheHttpImplConnPart"/>
		<platform:comprisesInterfacePart rdf:resource="&android-1_6;theOrgApacheHttpImplClientPart"/>
		<platform:comprisesInterfacePart rdf:resource="&android-1_6;theOrgApacheHttpImplAuthPart"/>
		<platform:comprisesInterfacePart rdf:resource="&android-1_6;theOrgApacheHttpImplEntityPart"/>
		<platform:comprisesInterfacePart rdf:resource="&android-1_6;theOrgApacheHttpImplPart"/>
		<platform:comprisesInterfacePart rdf:resource="&android-1_6;theOrgApacheHttpMessagePart"/>
		<platform:comprisesInterfacePart rdf:resource="&android-1_6;theOrgApacheHttpEntityPart"/>
		<platform:comprisesInterfacePart rdf:resource="&android-1_6;theOrgApacheHttpConnUtilPart"/>
		<platform:comprisesInterfacePart rdf:resource="&android-1_6;theOrgApacheHttpConnSslPart"/>
		<platform:comprisesInterfacePart rdf:resource="&android-1_6;theOrgApacheHttpConnRoutingPart"/>
		<platform:comprisesInterfacePart rdf:resource="&android-1_6;theOrgApacheHttpConnSchemePart"/>
		<platform:comprisesInterfacePart rdf:resource="&android-1_6;theOrgApacheHttpConnParamsPart"/>
		<platform:comprisesInterfacePart rdf:resource="&android-1_6;theOrgApacheHttpConnPart"/>
		<platform:comprisesInterfacePart rdf:resource="&android-1_6;theOrgApacheHttpCookieParamsPart"/>
		<platform:comprisesInterfacePart rdf:resource="&android-1_6;theOrgApacheHttpCookiePart"/>
		<platform:comprisesInterfacePart rdf:resource="&android-1_6;theOrgApacheHttpClientUtilsPart"/>
		<platform:comprisesInterfacePart rdf:resource="&android-1_6;theOrgApacheHttpClientProtocolPart"/>
		<platform:comprisesInterfacePart rdf:resource="&android-1_6;theOrgApacheHttpClientParamsPart"/>
		<platform:comprisesInterfacePart rdf:resource="&android-1_6;theOrgApacheHttpClientEntityPart"/>
		<platform:comprisesInterfacePart rdf:resource="&android-1_6;theOrgApacheHttpClientMethodsPart"/>
		<platform:comprisesInterfacePart rdf:resource="&android-1_6;theOrgApacheHttpClientPart"/>
		<platform:comprisesInterfacePart rdf:resource="&android-1_6;theOrgApacheHttpAuthParamsPart"/>
		<platform:comprisesInterfacePart rdf:resource="&android-1_6;theOrgApacheHttpAuthPart"/>
		<platform:comprisesInterfacePart rdf:resource="&android-1_6;theOrgApacheHttpParamsPart"/>
		<platform:comprisesInterfacePart rdf:resource="&android-1_6;theOrgApacheHttpUtilPart"/>
		<platform:comprisesInterfacePart rdf:resource="&android-1_6;theOrgApacheHttpProtocolPart"/>
		<platform:comprisesInterfacePart rdf:resource="&android-1_6;theOrgApacheHttpPart"/>
		<platform:comprisesInterfacePart rdf:resource="&android-1_6;theOrgApacheCommonsLoggingPart"/>
		<platform:comprisesInterfacePart rdf:resource="&android-1_6;theOrgW3cDomPart"/>
		<platform:comprisesInterfacePart rdf:resource="&android-1_6;theOrgXmlSaxExtPart"/>
		<platform:comprisesInterfacePart rdf:resource="&android-1_6;theOrgXmlSaxHelpersPart"/>
		<platform:comprisesInterfacePart rdf:resource="&android-1_6;theOrgXmlSaxPart"/>
		<platform:comprisesInterfacePart rdf:resource="&android-1_6;theOrgXmlpullV1Sax2Part"/>
		<platform:comprisesInterfacePart rdf:resource="&android-1_6;theOrgXmlpullV1Part"/>
		<platform:comprisesInterfacePart rdf:resource="&android-1_6;theJavaSqlPart"/>
		<platform:comprisesInterfacePart rdf:resource="&android-1_6;theJavaMathPart"/>
		<platform:comprisesInterfacePart rdf:resource="&android-1_6;theJavaBeansPart"/>
		<platform:comprisesInterfacePart rdf:resource="&android-1_6;theJavaAwtFontPart"/>
		<platform:comprisesInterfacePart rdf:resource="&android-1_6;theJavaTextPart"/>
		<platform:comprisesInterfacePart rdf:resource="&android-1_6;theJavaSecurityInterfacesPart"/>
		<platform:comprisesInterfacePart rdf:resource="&android-1_6;theJavaSecurityAclPart"/>
		<platform:comprisesInterfacePart rdf:resource="&android-1_6;theJavaSecuritySpecPart"/>
		<platform:comprisesInterfacePart rdf:resource="&android-1_6;theJavaSecurityCertPart"/>
		<platform:comprisesInterfacePart rdf:resource="&android-1_6;theJavaSecurityPart"/>
		<platform:comprisesInterfacePart rdf:resource="&android-1_6;theJavaNetPart"/>
		<platform:comprisesInterfacePart rdf:resource="&android-1_6;theJavaNioCharsetSpiPart"/>
		<platform:comprisesInterfacePart rdf:resource="&android-1_6;theJavaNioCharsetPart"/>
		<platform:comprisesInterfacePart rdf:resource="&android-1_6;theJavaNioChannelsSpiPart"/>
		<platform:comprisesInterfacePart rdf:resource="&android-1_6;theJavaNioChannelsPart"/>
		<platform:comprisesInterfacePart rdf:resource="&android-1_6;theJavaNioPart"/>
		<platform:comprisesInterfacePart rdf:resource="&android-1_6;theJavaIoPart"/>
		<platform:comprisesInterfacePart rdf:resource="&android-1_6;theJavaUtilPrefsPart"/>
		<platform:comprisesInterfacePart rdf:resource="&android-1_6;theJavaUtilLoggingPart"/>
		<platform:comprisesInterfacePart rdf:resource="&android-1_6;theJavaUtilZipPart"/>
		<platform:comprisesInterfacePart rdf:resource="&android-1_6;theJavaUtilJarPart"/>
		<platform:comprisesInterfacePart rdf:resource="&android-1_6;theJavaUtilRegexPart"/>
		<platform:comprisesInterfacePart rdf:resource="&android-1_6;theJavaUtilConcurrentLocksPart"/>
		<platform:comprisesInterfacePart rdf:resource="&android-1_6;theJavaUtilConcurrentAtomicPart"/>
		<platform:comprisesInterfacePart rdf:resource="&android-1_6;theJavaUtilConcurrentPart"/>
		<platform:comprisesInterfacePart rdf:resource="&android-1_6;theJavaUtilPart"/>
		<platform:comprisesInterfacePart rdf:resource="&android-1_6;theJavaLangRefPart"/>
		<platform:comprisesInterfacePart rdf:resource="&android-1_6;theJavaLangReflectPart"/>
		<platform:comprisesInterfacePart rdf:resource="&android-1_6;theJavaLangAnnotationPart"/>
		<platform:comprisesInterfacePart rdf:resource="&android-1_6;theJavaLangPart"/>
		<platform:comprisesInterfacePart rdf:resource="&android-1_6;theAndroidTestSuitebuilderAnnotationPart"/>
		<platform:comprisesInterfacePart rdf:resource="&android-1_6;theAndroidTestSuitebuilderPart"/>
		<platform:comprisesInterfacePart rdf:resource="&android-1_6;theAndroidTestMockPart"/>
		<platform:comprisesInterfacePart rdf:resource="&android-1_6;theAndroidTestPart"/>
		<platform:comprisesInterfacePart rdf:resource="&android-1_6;theAndroidTextUtilPart"/>
		<platform:comprisesInterfacePart rdf:resource="&android-1_6;theAndroidTextStylePart"/>
		<platform:comprisesInterfacePart rdf:resource="&android-1_6;theAndroidTextMethodPart"/>
		<platform:comprisesInterfacePart rdf:resource="&android-1_6;theAndroidTextFormatPart"/>
		<platform:comprisesInterfacePart rdf:resource="&android-1_6;theAndroidTextPart"/>
		<platform:comprisesInterfacePart rdf:resource="&android-1_6;theAndroidTelephonyGsmPart"/>
		<platform:comprisesInterfacePart rdf:resource="&android-1_6;theAndroidTelephonyPart"/>
		<platform:comprisesInterfacePart rdf:resource="&android-1_6;theAndroidSpeechTtsPart"/>
		<platform:comprisesInterfacePart rdf:resource="&android-1_6;theAndroidSpeechPart"/>
		<platform:comprisesInterfacePart rdf:resource="&android-1_6;theAndroidSaxPart"/>
		<platform:comprisesInterfacePart rdf:resource="&android-1_6;theAndroidWebkitPart"/>
		<platform:comprisesInterfacePart rdf:resource="&android-1_6;theAndroidProviderPart"/>
		<platform:comprisesInterfacePart rdf:resource="&android-1_6;theAndroidPreferencePart"/>
		<platform:comprisesInterfacePart rdf:resource="&android-1_6;theAndroidOpenglPart"/>
		<platform:comprisesInterfacePart rdf:resource="&android-1_6;theAndroidMediaPart"/>
		<platform:comprisesInterfacePart rdf:resource="&android-1_6;theAndroidLocationPart"/>
		<platform:comprisesInterfacePart rdf:resource="&android-1_6;theAndroidInputmethodservicePart"/>
		<platform:comprisesInterfacePart rdf:resource="&android-1_6;theAndroidHardwarePart"/>
		<platform:comprisesInterfacePart rdf:resource="&android-1_6;theAndroidGesturePart"/>
		<platform:comprisesInterfacePart rdf:resource="&android-1_6;theAndroidAppwidgetPart"/>
		<platform:comprisesInterfacePart rdf:resource="&android-1_6;theAndroidWidgetPart"/>
		<platform:comprisesInterfacePart rdf:resource="&android-1_6;theAndroidUtilPart"/>
		<platform:comprisesInterfacePart rdf:resource="&android-1_6;theAndroidDatabaseSqlitePart"/>
		<platform:comprisesInterfacePart rdf:resource="&android-1_6;theAndroidDatabasePart"/>
		<platform:comprisesInterfacePart rdf:resource="&android-1_6;theAndroidNetWifiPart"/>
		<platform:comprisesInterfacePart rdf:resource="&android-1_6;theAndroidNetHttpPart"/>
		<platform:comprisesInterfacePart rdf:resource="&android-1_6;theAndroidNetPart"/>
		<platform:comprisesInterfacePart rdf:resource="&android-1_6;theAndroidGraphicsDrawableShapesPart"/>
		<platform:comprisesInterfacePart rdf:resource="&android-1_6;theAndroidGraphicsDrawablePart"/>
		<platform:comprisesInterfacePart rdf:resource="&android-1_6;theAndroidGraphicsPart"/>
		<platform:comprisesInterfacePart rdf:resource="&android-1_6;theAndroidOsPart"/>
		<platform:comprisesInterfacePart rdf:resource="&android-1_6;theAndroidContentPmPart"/>
		<platform:comprisesInterfacePart rdf:resource="&android-1_6;theAndroidContentResPart"/>
		<platform:comprisesInterfacePart rdf:resource="&android-1_6;theAndroidContentPart"/>
		<platform:comprisesInterfacePart rdf:resource="&android-1_6;theAndroidViewAnimationPart"/>
		<platform:comprisesInterfacePart rdf:resource="&android-1_6;theAndroidViewInputmethodPart"/>
		<platform:comprisesInterfacePart rdf:resource="&android-1_6;theAndroidViewAccessibilityPart"/>
		<platform:comprisesInterfacePart rdf:resource="&android-1_6;theAndroidViewPart"/>
		<platform:comprisesInterfacePart rdf:resource="&android-1_6;theAndroidAppPart"/>
		<platform:comprisesInterfacePart rdf:resource="&android-1_6;theAndroidAccessibilityservicePart"/>
		<platform:comprisesInterfacePart rdf:resource="&android-1_6;theAndroidPart"/>
	</android-1_6:Android1_6API>
	<owl:Class rdf:about="&android-1_6;Android1_6VM">
		<owl:equivalentClass>
			<owl:Restriction>
				<owl:onProperty rdf:resource="&platform;implementsInterface"/>
				<owl:someValuesFrom rdf:resource="&android-1_6;Android1_6BytecodeFormat"/>
			</owl:Restriction>
		</owl:equivalentClass>
		<rdfs:subClassOf rdf:resource="&java;JavaVM"/>
		<rdfs:comment xml:lang="en">Android 1.6 virtual machine</rdfs:comment>
	</owl:Class>
	<owl:Class rdf:about="&android-1_6;Android1_6JRE">
		<owl:equivalentClass>
			<owl:Class >
				<owl:intersectionOf rdf:parseType="Collection">
					<owl:Restriction>
						<owl:onProperty rdf:resource="&platform;providesFeature"/>
						<owl:someValuesFrom rdf:resource="&android-1_6;Android1_6ClassLibrary"/>
					</owl:Restriction>
					<owl:Restriction>
						<owl:onProperty rdf:resource="&platform;providesFeature"/>
						<owl:someValuesFrom rdf:resource="&android-1_6;Android1_6VM"/>
					</owl:Restriction>
				</owl:intersectionOf>
			</owl:Class>
		</owl:equivalentClass>
		<rdfs:subClassOf rdf:resource="&java;JRE"/>
		<rdfs:comment xml:lang="en">Android 1.6 Java Runtime Environment</rdfs:comment>
	</owl:Class>
	<owl:Class rdf:about="&android-1_6;Android">
		<rdfs:subClassOf rdf:resource="&java;JavaAPIPart"/>
		<rdfs:seeAlso rdf:resource="&android-1_6;JavaLang"/>
		<rdfs:comment xml:lang="en">Java API part implementing the android package for Android 1.6</rdfs:comment>
	</owl:Class>
	<owl:Class rdf:about="&android-1_6;AndroidAccessibilityservice">
		<rdfs:subClassOf rdf:resource="&java;JavaAPIPart"/>
		<rdfs:seeAlso rdf:resource="&android-1_6;AndroidViewAccessibility"/>
		<rdfs:seeAlso rdf:resource="&android-1_6;JavaLang"/>
		<rdfs:seeAlso rdf:resource="&android-1_6;AndroidContent"/>
		<rdfs:seeAlso rdf:resource="&android-1_6;AndroidOs"/>
		<rdfs:seeAlso rdf:resource="&android-1_6;AndroidApp"/>
		<rdfs:comment xml:lang="en">Java API part implementing the android.accessibilityservice package for Android 1.6</rdfs:comment>
	</owl:Class>
	<owl:Class rdf:about="&android-1_6;AndroidApp">
		<rdfs:subClassOf rdf:resource="&android-1_5;AndroidApp"/>
		<rdfs:seeAlso rdf:resource="&android-1_6;AndroidGraphicsDrawable"/>
		<rdfs:seeAlso rdf:resource="&android-1_6;AndroidDatabase"/>
		<rdfs:seeAlso rdf:resource="&android-1_6;AndroidContent"/>
		<rdfs:seeAlso rdf:resource="&android-1_6;JavaUtil"/>
		<rdfs:seeAlso rdf:resource="&android-1_6;JavaIo"/>
		<rdfs:seeAlso rdf:resource="&android-1_6;AndroidView"/>
		<rdfs:seeAlso rdf:resource="&android-1_6;AndroidUtil"/>
		<rdfs:seeAlso rdf:resource="&android-1_6;AndroidNet"/>
		<rdfs:seeAlso rdf:resource="&android-1_6;AndroidGraphics"/>
		<rdfs:seeAlso rdf:resource="&android-1_6;AndroidContentRes"/>
		<rdfs:seeAlso rdf:resource="&android-1_6;AndroidWidget"/>
		<rdfs:seeAlso rdf:resource="&android-1_6;AndroidOs"/>
		<rdfs:seeAlso rdf:resource="&android-1_6;AndroidViewAccessibility"/>
		<rdfs:seeAlso rdf:resource="&android-1_6;AndroidContentPm"/>
		<rdfs:seeAlso rdf:resource="&android-1_6;JavaLang"/>
		<rdfs:comment xml:lang="en">Java API part implementing the android.app package for Android 1.6</rdfs:comment>
	</owl:Class>
	<owl:Class rdf:about="&android-1_6;AndroidView">
		<rdfs:subClassOf rdf:resource="&android-1_5;AndroidView"/>
		<rdfs:seeAlso rdf:resource="&android-1_6;AndroidContentRes"/>
		<rdfs:seeAlso rdf:resource="&android-1_6;AndroidHardware"/>
		<rdfs:seeAlso rdf:resource="&android-1_6;AndroidGraphicsDrawable"/>
		<rdfs:seeAlso rdf:resource="&android-1_6;AndroidViewInputmethod"/>
		<rdfs:seeAlso rdf:resource="&android-1_6;AndroidOs"/>
		<rdfs:seeAlso rdf:resource="&android-1_6;OrgXmlpullV1"/>
		<rdfs:seeAlso rdf:resource="&android-1_6;AndroidViewAccessibility"/>
		<rdfs:seeAlso rdf:resource="&android-1_6;AndroidContent"/>
		<rdfs:seeAlso rdf:resource="&android-1_6;JavaUtil"/>
		<rdfs:seeAlso rdf:resource="&android-1_6;JavaLang"/>
		<rdfs:seeAlso rdf:resource="&android-1_6;AndroidUtil"/>
		<rdfs:seeAlso rdf:resource="&android-1_6;AndroidNet"/>
		<rdfs:seeAlso rdf:resource="&android-1_6;JavaLangAnnotation"/>
		<rdfs:seeAlso rdf:resource="&android-1_6;AndroidGraphics"/>
		<rdfs:seeAlso rdf:resource="&android-1_6;AndroidViewAnimation"/>
		<rdfs:comment xml:lang="en">Java API part implementing the android.view package for Android 1.6</rdfs:comment>
	</owl:Class>
	<owl:Class rdf:about="&android-1_6;AndroidViewAccessibility">
		<rdfs:subClassOf rdf:resource="&java;JavaAPIPart"/>
		<rdfs:seeAlso rdf:resource="&android-1_6;JavaLang"/>
		<rdfs:seeAlso rdf:resource="&android-1_6;JavaUtil"/>
		<rdfs:seeAlso rdf:resource="&android-1_6;AndroidOs"/>
		<rdfs:comment xml:lang="en">Java API part implementing the android.view.accessibility package for Android 1.6</rdfs:comment>
	</owl:Class>
	<owl:Class rdf:about="&android-1_6;AndroidViewInputmethod">
		<owl:equivalentClass rdf:resource="&android-1_5;AndroidViewInputmethod"/>
		<rdfs:subClassOf rdf:resource="&java;JavaAPIPart"/>
		<rdfs:seeAlso rdf:resource="&android-1_6;AndroidGraphicsDrawable"/>
		<rdfs:seeAlso rdf:resource="&android-1_6;AndroidOs"/>
		<rdfs:seeAlso rdf:resource="&android-1_6;AndroidText"/>
		<rdfs:seeAlso rdf:resource="&android-1_6;AndroidContent"/>
		<rdfs:seeAlso rdf:resource="&android-1_6;JavaUtil"/>
		<rdfs:seeAlso rdf:resource="&android-1_6;AndroidView"/>
		<rdfs:seeAlso rdf:resource="&android-1_6;AndroidContentPm"/>
		<rdfs:seeAlso rdf:resource="&android-1_6;JavaLang"/>
		<rdfs:seeAlso rdf:resource="&android-1_6;AndroidUtil"/>
		<rdfs:seeAlso rdf:resource="&android-1_6;AndroidGraphics"/>
		<rdfs:comment xml:lang="en">Java API part implementing the android.view.inputmethod package for Android 1.6</rdfs:comment>
	</owl:Class>
	<owl:Class rdf:about="&android-1_6;AndroidViewAnimation">
		<rdfs:subClassOf rdf:resource="&android-1_5;AndroidViewAnimation"/>
		<rdfs:seeAlso rdf:resource="&android-1_6;JavaLang"/>
		<rdfs:seeAlso rdf:resource="&android-1_6;AndroidContent"/>
		<rdfs:seeAlso rdf:resource="&android-1_6;JavaUtil"/>
		<rdfs:seeAlso rdf:resource="&android-1_6;AndroidUtil"/>
		<rdfs:seeAlso rdf:resource="&android-1_6;AndroidView"/>
		<rdfs:seeAlso rdf:resource="&android-1_6;AndroidGraphics"/>
		<rdfs:comment xml:lang="en">Java API part implementing the android.view.animation package for Android 1.6</rdfs:comment>
	</owl:Class>
	<owl:Class rdf:about="&android-1_6;AndroidContent">
		<rdfs:subClassOf rdf:resource="&android-1_5;AndroidContent"/>
		<rdfs:seeAlso rdf:resource="&android-1_6;AndroidGraphicsDrawable"/>
		<rdfs:seeAlso rdf:resource="&android-1_6;OrgXmlpullV1"/>
		<rdfs:seeAlso rdf:resource="&android-1_6;AndroidDatabase"/>
		<rdfs:seeAlso rdf:resource="&android-1_6;JavaUtil"/>
		<rdfs:seeAlso rdf:resource="&android-1_6;JavaIo"/>
		<rdfs:seeAlso rdf:resource="&android-1_6;AndroidView"/>
		<rdfs:seeAlso rdf:resource="&android-1_6;AndroidDatabaseSqlite"/>
		<rdfs:seeAlso rdf:resource="&android-1_6;AndroidUtil"/>
		<rdfs:seeAlso rdf:resource="&android-1_6;AndroidNet"/>
		<rdfs:seeAlso rdf:resource="&android-1_6;AndroidGraphics"/>
		<rdfs:seeAlso rdf:resource="&android-1_6;AndroidContentRes"/>
		<rdfs:seeAlso rdf:resource="&android-1_6;AndroidOs"/>
		<rdfs:seeAlso rdf:resource="&android-1_6;AndroidContentPm"/>
		<rdfs:seeAlso rdf:resource="&android-1_6;JavaLang"/>
		<rdfs:comment xml:lang="en">Java API part implementing the android.content package for Android 1.6</rdfs:comment>
	</owl:Class>
	<owl:Class rdf:about="&android-1_6;AndroidContentRes">
		<rdfs:subClassOf rdf:resource="&android-1_5;AndroidContentRes"/>
		<rdfs:seeAlso rdf:resource="&android-1_6;JavaLang"/>
		<rdfs:seeAlso rdf:resource="&android-1_6;AndroidUtil"/>
		<rdfs:seeAlso rdf:resource="&android-1_6;AndroidGraphicsDrawable"/>
		<rdfs:seeAlso rdf:resource="&android-1_6;AndroidOs"/>
		<rdfs:seeAlso rdf:resource="&android-1_6;OrgXmlpullV1"/>
		<rdfs:seeAlso rdf:resource="&android-1_6;JavaUtil"/>
		<rdfs:seeAlso rdf:resource="&android-1_6;JavaIo"/>
		<rdfs:seeAlso rdf:resource="&android-1_6;AndroidGraphics"/>
		<rdfs:comment xml:lang="en">Java API part implementing the android.content.res package for Android 1.6</rdfs:comment>
	</owl:Class>
	<owl:Class rdf:about="&android-1_6;AndroidContentPm">
		<rdfs:subClassOf rdf:resource="&java;JavaAPIPart"/>
		<rdfs:seeAlso rdf:resource="&android-1_6;JavaLang"/>
		<rdfs:seeAlso rdf:resource="&android-1_6;AndroidContentRes"/>
		<rdfs:seeAlso rdf:resource="&android-1_6;AndroidUtil"/>
		<rdfs:seeAlso rdf:resource="&android-1_6;AndroidGraphicsDrawable"/>
		<rdfs:seeAlso rdf:resource="&android-1_6;AndroidOs"/>
		<rdfs:seeAlso rdf:resource="&android-1_6;AndroidContent"/>
		<rdfs:seeAlso rdf:resource="&android-1_6;JavaUtil"/>
		<rdfs:comment xml:lang="en">Java API part implementing the android.content.pm package for Android 1.6</rdfs:comment>
	</owl:Class>
	<owl:Class rdf:about="&android-1_6;AndroidOs">
		<rdfs:subClassOf rdf:resource="&android-1_5;AndroidOs"/>
		<rdfs:seeAlso rdf:resource="&android-1_6;JavaNet"/>
		<rdfs:seeAlso rdf:resource="&android-1_6;JavaUtil"/>
		<rdfs:seeAlso rdf:resource="&android-1_6;JavaIo"/>
		<rdfs:seeAlso rdf:resource="&android-1_6;JavaLang"/>
		<rdfs:seeAlso rdf:resource="&android-1_6;AndroidUtil"/>
		<rdfs:seeAlso rdf:resource="&android-1_6;JavaUtilConcurrent"/>
		<rdfs:comment xml:lang="en">Java API part implementing the android.os package for Android 1.6</rdfs:comment>
	</owl:Class>
	<owl:Class rdf:about="&android-1_6;AndroidGraphics">
		<rdfs:subClassOf rdf:resource="&android-1_5;AndroidGraphics"/>
		<rdfs:seeAlso rdf:resource="&android-1_6;JavaNio"/>
		<rdfs:seeAlso rdf:resource="&android-1_6;JavaLang"/>
		<rdfs:seeAlso rdf:resource="&android-1_6;AndroidContentRes"/>
		<rdfs:seeAlso rdf:resource="&android-1_6;AndroidUtil"/>
		<rdfs:seeAlso rdf:resource="&android-1_6;AndroidOs"/>
		<rdfs:seeAlso rdf:resource="&android-1_6;JavaxMicroeditionKhronosOpengles"/>
		<rdfs:seeAlso rdf:resource="&android-1_6;JavaIo"/>
		<rdfs:comment xml:lang="en">Java API part implementing the android.graphics package for Android 1.6</rdfs:comment>
	</owl:Class>
	<owl:Class rdf:about="&android-1_6;AndroidGraphicsDrawable">
		<rdfs:subClassOf rdf:resource="&android-1_5;AndroidGraphicsDrawable"/>
		<rdfs:seeAlso rdf:resource="&android-1_6;AndroidGraphicsDrawableShapes"/>
		<rdfs:seeAlso rdf:resource="&android-1_6;JavaLang"/>
		<rdfs:seeAlso rdf:resource="&android-1_6;AndroidContentRes"/>
		<rdfs:seeAlso rdf:resource="&android-1_6;AndroidUtil"/>
		<rdfs:seeAlso rdf:resource="&android-1_6;OrgXmlpullV1"/>
		<rdfs:seeAlso rdf:resource="&android-1_6;JavaIo"/>
		<rdfs:seeAlso rdf:resource="&android-1_6;AndroidGraphics"/>
		<rdfs:comment xml:lang="en">Java API part implementing the android.graphics.drawable package for Android 1.6</rdfs:comment>
	</owl:Class>
	<owl:Class rdf:about="&android-1_6;AndroidGraphicsDrawableShapes">
		<owl:equivalentClass rdf:resource="&android-1_5;AndroidGraphicsDrawableShapes"/>
		<rdfs:subClassOf rdf:resource="&java;JavaAPIPart"/>
		<rdfs:seeAlso rdf:resource="&android-1_6;JavaLang"/>
		<rdfs:seeAlso rdf:resource="&android-1_6;AndroidGraphics"/>
		<rdfs:comment xml:lang="en">Java API part implementing the android.graphics.drawable.shapes package for Android 1.6</rdfs:comment>
	</owl:Class>
	<owl:Class rdf:about="&android-1_6;AndroidNet">
		<owl:equivalentClass rdf:resource="&android-1_5;AndroidNet"/>
		<rdfs:subClassOf rdf:resource="&java;JavaAPIPart"/>
		<rdfs:seeAlso rdf:resource="&android-1_6;JavaLang"/>
		<rdfs:seeAlso rdf:resource="&android-1_6;JavaxNetSsl"/>
		<rdfs:seeAlso rdf:resource="&android-1_6;JavaNet"/>
		<rdfs:seeAlso rdf:resource="&android-1_6;AndroidOs"/>
		<rdfs:seeAlso rdf:resource="&android-1_6;AndroidContent"/>
		<rdfs:seeAlso rdf:resource="&android-1_6;JavaUtil"/>
		<rdfs:seeAlso rdf:resource="&android-1_6;JavaIo"/>
		<rdfs:seeAlso rdf:resource="&android-1_6;JavaxNet"/>
		<rdfs:comment xml:lang="en">Java API part implementing the android.net package for Android 1.6</rdfs:comment>
	</owl:Class>
	<owl:Class rdf:about="&android-1_6;AndroidNetHttp">
		<owl:equivalentClass rdf:resource="&android-1_5;AndroidNetHttp"/>
		<rdfs:subClassOf rdf:resource="&java;JavaAPIPart"/>
		<rdfs:seeAlso rdf:resource="&android-1_6;JavaLang"/>
		<rdfs:seeAlso rdf:resource="&android-1_6;JavaSecurityCert"/>
		<rdfs:seeAlso rdf:resource="&android-1_6;AndroidOs"/>
		<rdfs:comment xml:lang="en">Java API part implementing the android.net.http package for Android 1.6</rdfs:comment>
	</owl:Class>
	<owl:Class rdf:about="&android-1_6;AndroidNetWifi">
		<rdfs:subClassOf rdf:resource="&android-1_5;AndroidNetWifi"/>
		<rdfs:seeAlso rdf:resource="&android-1_6;JavaLang"/>
		<rdfs:seeAlso rdf:resource="&android-1_6;JavaUtil"/>
		<rdfs:seeAlso rdf:resource="&android-1_6;AndroidOs"/>
		<rdfs:seeAlso rdf:resource="&android-1_6;AndroidNet"/>
		<rdfs:comment xml:lang="en">Java API part implementing the android.net.wifi package for Android 1.6</rdfs:comment>
	</owl:Class>
	<owl:Class rdf:about="&android-1_6;AndroidDatabase">
		<owl:equivalentClass rdf:resource="&android-1_5;AndroidDatabase"/>
		<rdfs:subClassOf rdf:resource="&java;JavaAPIPart"/>
		<rdfs:seeAlso rdf:resource="&android-1_6;AndroidOs"/>
		<rdfs:seeAlso rdf:resource="&android-1_6;AndroidContent"/>
		<rdfs:seeAlso rdf:resource="&android-1_6;JavaUtil"/>
		<rdfs:seeAlso rdf:resource="&android-1_6;JavaIo"/>
		<rdfs:seeAlso rdf:resource="&android-1_6;AndroidDatabaseSqlite"/>
		<rdfs:seeAlso rdf:resource="&android-1_6;JavaLang"/>
		<rdfs:seeAlso rdf:resource="&android-1_6;AndroidNet"/>
		<rdfs:comment xml:lang="en">Java API part implementing the android.database package for Android 1.6</rdfs:comment>
	</owl:Class>
	<owl:Class rdf:about="&android-1_6;AndroidDatabaseSqlite">
		<owl:equivalentClass rdf:resource="&android-1_5;AndroidDatabaseSqlite"/>
		<rdfs:subClassOf rdf:resource="&java;JavaAPIPart"/>
		<rdfs:seeAlso rdf:resource="&android-1_6;JavaLang"/>
		<rdfs:seeAlso rdf:resource="&android-1_6;AndroidDatabase"/>
		<rdfs:seeAlso rdf:resource="&android-1_6;AndroidContent"/>
		<rdfs:seeAlso rdf:resource="&android-1_6;JavaUtil"/>
		<rdfs:seeAlso rdf:resource="&android-1_6;JavaIo"/>
		<rdfs:comment xml:lang="en">Java API part implementing the android.database.sqlite package for Android 1.6</rdfs:comment>
	</owl:Class>
	<owl:Class rdf:about="&android-1_6;AndroidUtil">
		<rdfs:subClassOf rdf:resource="&android-1_5;AndroidUtil"/>
		<rdfs:seeAlso rdf:resource="&android-1_6;JavaLang"/>
		<rdfs:seeAlso rdf:resource="&android-1_6;OrgXmlpullV1"/>
		<rdfs:seeAlso rdf:resource="&android-1_6;JavaUtil"/>
		<rdfs:seeAlso rdf:resource="&android-1_6;JavaIo"/>
		<rdfs:seeAlso rdf:resource="&android-1_6;OrgXmlSax"/>
		<rdfs:comment xml:lang="en">Java API part implementing the android.util package for Android 1.6</rdfs:comment>
	</owl:Class>
	<owl:Class rdf:about="&android-1_6;AndroidWidget">
		<rdfs:subClassOf rdf:resource="&android-1_5;AndroidWidget"/>
		<rdfs:seeAlso rdf:resource="&android-1_6;AndroidGraphicsDrawable"/>
		<rdfs:seeAlso rdf:resource="&android-1_6;AndroidApp"/>
		<rdfs:seeAlso rdf:resource="&android-1_6;AndroidText"/>
		<rdfs:seeAlso rdf:resource="&android-1_6;AndroidDatabase"/>
		<rdfs:seeAlso rdf:resource="&android-1_6;AndroidContent"/>
		<rdfs:seeAlso rdf:resource="&android-1_6;JavaUtil"/>
		<rdfs:seeAlso rdf:resource="&android-1_6;AndroidView"/>
		<rdfs:seeAlso rdf:resource="&android-1_6;AndroidTextMethod"/>
		<rdfs:seeAlso rdf:resource="&android-1_6;AndroidUtil"/>
		<rdfs:seeAlso rdf:resource="&android-1_6;AndroidNet"/>
		<rdfs:seeAlso rdf:resource="&android-1_6;AndroidGraphics"/>
		<rdfs:seeAlso rdf:resource="&android-1_6;AndroidViewAnimation"/>
		<rdfs:seeAlso rdf:resource="&android-1_6;AndroidContentRes"/>
		<rdfs:seeAlso rdf:resource="&android-1_6;AndroidOs"/>
		<rdfs:seeAlso rdf:resource="&android-1_6;AndroidViewInputmethod"/>
		<rdfs:seeAlso rdf:resource="&android-1_6;AndroidViewAccessibility"/>
		<rdfs:seeAlso rdf:resource="&android-1_6;AndroidMedia"/>
		<rdfs:seeAlso rdf:resource="&android-1_6;JavaLang"/>
		<rdfs:seeAlso rdf:resource="&android-1_6;JavaLangAnnotation"/>
		<rdfs:comment xml:lang="en">Java API part implementing the android.widget package for Android 1.6</rdfs:comment>
	</owl:Class>
	<owl:Class rdf:about="&android-1_6;AndroidAppwidget">
		<rdfs:subClassOf rdf:resource="&android-1_5;AndroidAppwidget"/>
		<rdfs:seeAlso rdf:resource="&android-1_6;JavaLang"/>
		<rdfs:seeAlso rdf:resource="&android-1_6;AndroidUtil"/>
		<rdfs:seeAlso rdf:resource="&android-1_6;AndroidWidget"/>
		<rdfs:seeAlso rdf:resource="&android-1_6;AndroidOs"/>
		<rdfs:seeAlso rdf:resource="&android-1_6;AndroidContent"/>
		<rdfs:seeAlso rdf:resource="&android-1_6;JavaUtil"/>
		<rdfs:seeAlso rdf:resource="&android-1_6;AndroidView"/>
		<rdfs:seeAlso rdf:resource="&android-1_6;AndroidGraphics"/>
		<rdfs:comment xml:lang="en">Java API part implementing the android.appwidget package for Android 1.6</rdfs:comment>
	</owl:Class>
	<owl:Class rdf:about="&android-1_6;AndroidGesture">
		<rdfs:subClassOf rdf:resource="&java;JavaAPIPart"/>
		<rdfs:seeAlso rdf:resource="&android-1_6;JavaLang"/>
		<rdfs:seeAlso rdf:resource="&android-1_6;AndroidUtil"/>
		<rdfs:seeAlso rdf:resource="&android-1_6;AndroidWidget"/>
		<rdfs:seeAlso rdf:resource="&android-1_6;AndroidOs"/>
		<rdfs:seeAlso rdf:resource="&android-1_6;AndroidContent"/>
		<rdfs:seeAlso rdf:resource="&android-1_6;JavaUtil"/>
		<rdfs:seeAlso rdf:resource="&android-1_6;JavaIo"/>
		<rdfs:seeAlso rdf:resource="&android-1_6;AndroidView"/>
		<rdfs:seeAlso rdf:resource="&android-1_6;AndroidGraphics"/>
		<rdfs:comment xml:lang="en">Java API part implementing the android.gesture package for Android 1.6</rdfs:comment>
	</owl:Class>
	<owl:Class rdf:about="&android-1_6;AndroidHardware">
		<owl:equivalentClass rdf:resource="&android-1_5;AndroidHardware"/>
		<rdfs:subClassOf rdf:resource="&java;JavaAPIPart"/>
		<rdfs:seeAlso rdf:resource="&android-1_6;JavaLang"/>
		<rdfs:seeAlso rdf:resource="&android-1_6;JavaUtil"/>
		<rdfs:seeAlso rdf:resource="&android-1_6;AndroidView"/>
		<rdfs:seeAlso rdf:resource="&android-1_6;AndroidOs"/>
		<rdfs:comment xml:lang="en">Java API part implementing the android.hardware package for Android 1.6</rdfs:comment>
	</owl:Class>
	<owl:Class rdf:about="&android-1_6;AndroidInputmethodservice">
		<rdfs:subClassOf rdf:resource="&android-1_5;AndroidInputmethodservice"/>
		<rdfs:seeAlso rdf:resource="&android-1_6;AndroidContentRes"/>
		<rdfs:seeAlso rdf:resource="&android-1_6;AndroidGraphicsDrawable"/>
		<rdfs:seeAlso rdf:resource="&android-1_6;AndroidWidget"/>
		<rdfs:seeAlso rdf:resource="&android-1_6;AndroidViewInputmethod"/>
		<rdfs:seeAlso rdf:resource="&android-1_6;AndroidOs"/>
		<rdfs:seeAlso rdf:resource="&android-1_6;AndroidApp"/>
		<rdfs:seeAlso rdf:resource="&android-1_6;AndroidContent"/>
		<rdfs:seeAlso rdf:resource="&android-1_6;JavaUtil"/>
		<rdfs:seeAlso rdf:resource="&android-1_6;JavaIo"/>
		<rdfs:seeAlso rdf:resource="&android-1_6;AndroidView"/>
		<rdfs:seeAlso rdf:resource="&android-1_6;JavaLang"/>
		<rdfs:seeAlso rdf:resource="&android-1_6;AndroidUtil"/>
		<rdfs:seeAlso rdf:resource="&android-1_6;AndroidGraphics"/>
		<rdfs:comment xml:lang="en">Java API part implementing the android.inputmethodservice package for Android 1.6</rdfs:comment>
	</owl:Class>
	<owl:Class rdf:about="&android-1_6;AndroidLocation">
		<rdfs:subClassOf rdf:resource="&android-1_5;AndroidLocation"/>
		<rdfs:seeAlso rdf:resource="&android-1_6;JavaLang"/>
		<rdfs:seeAlso rdf:resource="&android-1_6;AndroidUtil"/>
		<rdfs:seeAlso rdf:resource="&android-1_6;AndroidOs"/>
		<rdfs:seeAlso rdf:resource="&android-1_6;AndroidApp"/>
		<rdfs:seeAlso rdf:resource="&android-1_6;AndroidContent"/>
		<rdfs:seeAlso rdf:resource="&android-1_6;JavaUtil"/>
		<rdfs:comment xml:lang="en">Java API part implementing the android.location package for Android 1.6</rdfs:comment>
	</owl:Class>
	<owl:Class rdf:about="&android-1_6;AndroidMedia">
		<rdfs:subClassOf rdf:resource="&android-1_5;AndroidMedia"/>
		<rdfs:seeAlso rdf:resource="&android-1_6;JavaNio"/>
		<rdfs:seeAlso rdf:resource="&android-1_6;JavaLang"/>
		<rdfs:seeAlso rdf:resource="&android-1_6;AndroidContentRes"/>
		<rdfs:seeAlso rdf:resource="&android-1_6;AndroidHardware"/>
		<rdfs:seeAlso rdf:resource="&android-1_6;AndroidOs"/>
		<rdfs:seeAlso rdf:resource="&android-1_6;AndroidNet"/>
		<rdfs:seeAlso rdf:resource="&android-1_6;AndroidApp"/>
		<rdfs:seeAlso rdf:resource="&android-1_6;AndroidDatabase"/>
		<rdfs:seeAlso rdf:resource="&android-1_6;AndroidContent"/>
		<rdfs:seeAlso rdf:resource="&android-1_6;JavaIo"/>
		<rdfs:seeAlso rdf:resource="&android-1_6;AndroidView"/>
		<rdfs:seeAlso rdf:resource="&android-1_6;AndroidGraphics"/>
		<rdfs:comment xml:lang="en">Java API part implementing the android.media package for Android 1.6</rdfs:comment>
	</owl:Class>
	<owl:Class rdf:about="&android-1_6;AndroidOpengl">
		<rdfs:subClassOf rdf:resource="&android-1_5;AndroidOpengl"/>
		<rdfs:seeAlso rdf:resource="&android-1_6;JavaNio"/>
		<rdfs:seeAlso rdf:resource="&android-1_6;JavaxMicroeditionKhronosEgl"/>
		<rdfs:seeAlso rdf:resource="&android-1_6;JavaLang"/>
		<rdfs:seeAlso rdf:resource="&android-1_6;AndroidUtil"/>
		<rdfs:seeAlso rdf:resource="&android-1_6;AndroidContent"/>
		<rdfs:seeAlso rdf:resource="&android-1_6;JavaxMicroeditionKhronosOpengles"/>
		<rdfs:seeAlso rdf:resource="&android-1_6;JavaIo"/>
		<rdfs:seeAlso rdf:resource="&android-1_6;AndroidView"/>
		<rdfs:seeAlso rdf:resource="&android-1_6;AndroidGraphics"/>
		<rdfs:comment xml:lang="en">Java API part implementing the android.opengl package for Android 1.6</rdfs:comment>
	</owl:Class>
	<owl:Class rdf:about="&android-1_6;AndroidPreference">
		<rdfs:subClassOf rdf:resource="&android-1_5;AndroidPreference"/>
		<rdfs:seeAlso rdf:resource="&android-1_6;AndroidContentRes"/>
		<rdfs:seeAlso rdf:resource="&android-1_6;AndroidGraphicsDrawable"/>
		<rdfs:seeAlso rdf:resource="&android-1_6;AndroidWidget"/>
		<rdfs:seeAlso rdf:resource="&android-1_6;AndroidOs"/>
		<rdfs:seeAlso rdf:resource="&android-1_6;AndroidApp"/>
		<rdfs:seeAlso rdf:resource="&android-1_6;AndroidContent"/>
		<rdfs:seeAlso rdf:resource="&android-1_6;AndroidView"/>
		<rdfs:seeAlso rdf:resource="&android-1_6;JavaLang"/>
		<rdfs:seeAlso rdf:resource="&android-1_6;AndroidUtil"/>
		<rdfs:seeAlso rdf:resource="&android-1_6;AndroidNet"/>
		<rdfs:comment xml:lang="en">Java API part implementing the android.preference package for Android 1.6</rdfs:comment>
	</owl:Class>
	<owl:Class rdf:about="&android-1_6;AndroidProvider">
		<rdfs:subClassOf rdf:resource="&android-1_5;AndroidProvider"/>
		<rdfs:seeAlso rdf:resource="&android-1_6;JavaLang"/>
		<rdfs:seeAlso rdf:resource="&android-1_6;AndroidContentRes"/>
		<rdfs:seeAlso rdf:resource="&android-1_6;AndroidUtil"/>
		<rdfs:seeAlso rdf:resource="&android-1_6;AndroidNet"/>
		<rdfs:seeAlso rdf:resource="&android-1_6;AndroidDatabase"/>
		<rdfs:seeAlso rdf:resource="&android-1_6;AndroidWebkit"/>
		<rdfs:seeAlso rdf:resource="&android-1_6;AndroidContent"/>
		<rdfs:seeAlso rdf:resource="&android-1_6;JavaIo"/>
		<rdfs:seeAlso rdf:resource="&android-1_6;AndroidGraphics"/>
		<rdfs:comment xml:lang="en">Java API part implementing the android.provider package for Android 1.6</rdfs:comment>
	</owl:Class>
	<owl:Class rdf:about="&android-1_6;AndroidWebkit">
		<rdfs:subClassOf rdf:resource="&android-1_5;AndroidWebkit"/>
		<rdfs:seeAlso rdf:resource="&android-1_6;AndroidWidget"/>
		<rdfs:seeAlso rdf:resource="&android-1_6;AndroidOs"/>
		<rdfs:seeAlso rdf:resource="&android-1_6;AndroidContent"/>
		<rdfs:seeAlso rdf:resource="&android-1_6;JavaUtil"/>
		<rdfs:seeAlso rdf:resource="&android-1_6;JavaIo"/>
		<rdfs:seeAlso rdf:resource="&android-1_6;AndroidView"/>
		<rdfs:seeAlso rdf:resource="&android-1_6;JavaLang"/>
		<rdfs:seeAlso rdf:resource="&android-1_6;AndroidUtil"/>
		<rdfs:seeAlso rdf:resource="&android-1_6;AndroidNetHttp"/>
		<rdfs:seeAlso rdf:resource="&android-1_6;AndroidGraphics"/>
		<rdfs:comment xml:lang="en">Java API part implementing the android.webkit package for Android 1.6</rdfs:comment>
	</owl:Class>
	<owl:Class rdf:about="&android-1_6;AndroidSax">
		<owl:equivalentClass rdf:resource="&android-1_5;AndroidSax"/>
		<rdfs:subClassOf rdf:resource="&java;JavaAPIPart"/>
		<rdfs:seeAlso rdf:resource="&android-1_6;JavaLang"/>
		<rdfs:seeAlso rdf:resource="&android-1_6;OrgXmlSax"/>
		<rdfs:comment xml:lang="en">Java API part implementing the android.sax package for Android 1.6</rdfs:comment>
	</owl:Class>
	<owl:Class rdf:about="&android-1_6;AndroidSpeech">
		<owl:equivalentClass rdf:resource="&android-1_5;AndroidSpeech"/>
		<rdfs:subClassOf rdf:resource="&java;JavaAPIPart"/>
		<rdfs:seeAlso rdf:resource="&android-1_6;JavaLang"/>
		<rdfs:comment xml:lang="en">Java API part implementing the android.speech package for Android 1.6</rdfs:comment>
	</owl:Class>
	<owl:Class rdf:about="&android-1_6;AndroidSpeechTts">
		<rdfs:subClassOf rdf:resource="&java;JavaAPIPart"/>
		<rdfs:seeAlso rdf:resource="&android-1_6;JavaLang"/>
		<rdfs:seeAlso rdf:resource="&android-1_6;AndroidContent"/>
		<rdfs:seeAlso rdf:resource="&android-1_6;JavaUtil"/>
		<rdfs:comment xml:lang="en">Java API part implementing the android.speech.tts package for Android 1.6</rdfs:comment>
	</owl:Class>
	<owl:Class rdf:about="&android-1_6;AndroidTelephony">
		<rdfs:subClassOf rdf:resource="&android-1_5;AndroidTelephony"/>
		<rdfs:seeAlso rdf:resource="&android-1_6;JavaLang"/>
		<rdfs:seeAlso rdf:resource="&android-1_6;AndroidOs"/>
		<rdfs:seeAlso rdf:resource="&android-1_6;AndroidApp"/>
		<rdfs:seeAlso rdf:resource="&android-1_6;AndroidText"/>
		<rdfs:seeAlso rdf:resource="&android-1_6;AndroidContent"/>
		<rdfs:seeAlso rdf:resource="&android-1_6;JavaUtil"/>
		<rdfs:comment xml:lang="en">Java API part implementing the android.telephony package for Android 1.6</rdfs:comment>
	</owl:Class>
	<owl:Class rdf:about="&android-1_6;AndroidTelephonyGsm">
		<rdfs:subClassOf rdf:resource="&java;JavaAPIPart"/>
		<rdfs:seeAlso rdf:resource="&android-1_6;AndroidTelephony"/>
		<rdfs:seeAlso rdf:resource="&android-1_6;JavaLang"/>
		<rdfs:seeAlso rdf:resource="&android-1_6;JavaUtil"/>
		<rdfs:seeAlso rdf:resource="&android-1_6;AndroidOs"/>
		<rdfs:seeAlso rdf:resource="&android-1_6;AndroidApp"/>
		<rdfs:comment xml:lang="en">Java API part implementing the android.telephony.gsm package for Android 1.6</rdfs:comment>
	</owl:Class>
	<owl:Class rdf:about="&android-1_6;AndroidText">
		<owl:equivalentClass rdf:resource="&android-1_5;AndroidText"/>
		<rdfs:subClassOf rdf:resource="&java;JavaAPIPart"/>
		<rdfs:seeAlso rdf:resource="&android-1_6;JavaLang"/>
		<rdfs:seeAlso rdf:resource="&android-1_6;JavaUtilRegex"/>
		<rdfs:seeAlso rdf:resource="&android-1_6;AndroidUtil"/>
		<rdfs:seeAlso rdf:resource="&android-1_6;AndroidGraphicsDrawable"/>
		<rdfs:seeAlso rdf:resource="&android-1_6;AndroidOs"/>
		<rdfs:seeAlso rdf:resource="&android-1_6;JavaUtil"/>
		<rdfs:seeAlso rdf:resource="&android-1_6;AndroidView"/>
		<rdfs:seeAlso rdf:resource="&android-1_6;OrgXmlSax"/>
		<rdfs:seeAlso rdf:resource="&android-1_6;AndroidGraphics"/>
		<rdfs:comment xml:lang="en">Java API part implementing the android.text package for Android 1.6</rdfs:comment>
	</owl:Class>
	<owl:Class rdf:about="&android-1_6;AndroidTextFormat">
		<owl:equivalentClass rdf:resource="&android-1_5;AndroidTextFormat"/>
		<rdfs:subClassOf rdf:resource="&java;JavaAPIPart"/>
		<rdfs:seeAlso rdf:resource="&android-1_6;JavaLang"/>
		<rdfs:seeAlso rdf:resource="&android-1_6;JavaText"/>
		<rdfs:seeAlso rdf:resource="&android-1_6;AndroidContent"/>
		<rdfs:seeAlso rdf:resource="&android-1_6;JavaUtil"/>
		<rdfs:comment xml:lang="en">Java API part implementing the android.text.format package for Android 1.6</rdfs:comment>
	</owl:Class>
	<owl:Class rdf:about="&android-1_6;AndroidTextMethod">
		<rdfs:subClassOf rdf:resource="&android-1_5;AndroidTextMethod"/>
		<rdfs:seeAlso rdf:resource="&android-1_6;JavaLang"/>
		<rdfs:seeAlso rdf:resource="&android-1_6;AndroidWidget"/>
		<rdfs:seeAlso rdf:resource="&android-1_6;AndroidOs"/>
		<rdfs:seeAlso rdf:resource="&android-1_6;AndroidApp"/>
		<rdfs:seeAlso rdf:resource="&android-1_6;AndroidText"/>
		<rdfs:seeAlso rdf:resource="&android-1_6;AndroidContent"/>
		<rdfs:seeAlso rdf:resource="&android-1_6;AndroidView"/>
		<rdfs:seeAlso rdf:resource="&android-1_6;AndroidGraphics"/>
		<rdfs:comment xml:lang="en">Java API part implementing the android.text.method package for Android 1.6</rdfs:comment>
	</owl:Class>
	<owl:Class rdf:about="&android-1_6;AndroidTextStyle">
		<rdfs:subClassOf rdf:resource="&android-1_5;AndroidTextStyle"/>
		<rdfs:seeAlso rdf:resource="&android-1_6;JavaLang"/>
		<rdfs:seeAlso rdf:resource="&android-1_6;AndroidContentRes"/>
		<rdfs:seeAlso rdf:resource="&android-1_6;AndroidGraphicsDrawable"/>
		<rdfs:seeAlso rdf:resource="&android-1_6;AndroidOs"/>
		<rdfs:seeAlso rdf:resource="&android-1_6;AndroidNet"/>
		<rdfs:seeAlso rdf:resource="&android-1_6;AndroidText"/>
		<rdfs:seeAlso rdf:resource="&android-1_6;AndroidContent"/>
		<rdfs:seeAlso rdf:resource="&android-1_6;AndroidView"/>
		<rdfs:seeAlso rdf:resource="&android-1_6;AndroidGraphics"/>
		<rdfs:comment xml:lang="en">Java API part implementing the android.text.style package for Android 1.6</rdfs:comment>
	</owl:Class>
	<owl:Class rdf:about="&android-1_6;AndroidTextUtil">
		<owl:equivalentClass rdf:resource="&android-1_5;AndroidTextUtil"/>
		<rdfs:subClassOf rdf:resource="&java;JavaAPIPart"/>
		<rdfs:seeAlso rdf:resource="&android-1_6;AndroidText"/>
		<rdfs:seeAlso rdf:resource="&android-1_6;JavaLang"/>
		<rdfs:seeAlso rdf:resource="&android-1_6;JavaUtilRegex"/>
		<rdfs:seeAlso rdf:resource="&android-1_6;AndroidWidget"/>
		<rdfs:comment xml:lang="en">Java API part implementing the android.text.util package for Android 1.6</rdfs:comment>
	</owl:Class>
	<owl:Class rdf:about="&android-1_6;AndroidTest">
		<rdfs:subClassOf rdf:resource="&android-1_5;AndroidTest"/>
		<rdfs:seeAlso rdf:resource="&android-1_6;JavaUtilRegex"/>
		<rdfs:seeAlso rdf:resource="&android-1_6;JunitRunner"/>
		<rdfs:seeAlso rdf:resource="&android-1_6;AndroidOs"/>
		<rdfs:seeAlso rdf:resource="&android-1_6;AndroidApp"/>
		<rdfs:seeAlso rdf:resource="&android-1_6;AndroidContent"/>
		<rdfs:seeAlso rdf:resource="&android-1_6;JavaUtil"/>
		<rdfs:seeAlso rdf:resource="&android-1_6;JavaIo"/>
		<rdfs:seeAlso rdf:resource="&android-1_6;AndroidView"/>
		<rdfs:seeAlso rdf:resource="&android-1_6;AndroidDatabaseSqlite"/>
		<rdfs:seeAlso rdf:resource="&android-1_6;JavaLang"/>
		<rdfs:seeAlso rdf:resource="&android-1_6;AndroidNet"/>
		<rdfs:seeAlso rdf:resource="&android-1_6;JunitFramework"/>
		<rdfs:seeAlso rdf:resource="&android-1_6;AndroidTestMock"/>
		<rdfs:seeAlso rdf:resource="&android-1_6;JavaLangAnnotation"/>
		<rdfs:comment xml:lang="en">Java API part implementing the android.test package for Android 1.6</rdfs:comment>
	</owl:Class>
	<owl:Class rdf:about="&android-1_6;AndroidTestMock">
		<rdfs:subClassOf rdf:resource="&java;JavaAPIPart"/>
		<rdfs:seeAlso rdf:resource="&android-1_6;AndroidGraphicsDrawable"/>
		<rdfs:seeAlso rdf:resource="&android-1_6;AndroidApp"/>
		<rdfs:seeAlso rdf:resource="&android-1_6;AndroidDatabase"/>
		<rdfs:seeAlso rdf:resource="&android-1_6;AndroidContent"/>
		<rdfs:seeAlso rdf:resource="&android-1_6;JavaUtil"/>
		<rdfs:seeAlso rdf:resource="&android-1_6;JavaIo"/>
		<rdfs:seeAlso rdf:resource="&android-1_6;AndroidDatabaseSqlite"/>
		<rdfs:seeAlso rdf:resource="&android-1_6;AndroidUtil"/>
		<rdfs:seeAlso rdf:resource="&android-1_6;AndroidNet"/>
		<rdfs:seeAlso rdf:resource="&android-1_6;AndroidGraphics"/>
		<rdfs:seeAlso rdf:resource="&android-1_6;AndroidContentRes"/>
		<rdfs:seeAlso rdf:resource="&android-1_6;AndroidOs"/>
		<rdfs:seeAlso rdf:resource="&android-1_6;AndroidContentPm"/>
		<rdfs:seeAlso rdf:resource="&android-1_6;JavaLang"/>
		<rdfs:comment xml:lang="en">Java API part implementing the android.test.mock package for Android 1.6</rdfs:comment>
	</owl:Class>
	<owl:Class rdf:about="&android-1_6;AndroidTestSuitebuilder">
		<owl:equivalentClass rdf:resource="&android-1_5;AndroidTestSuitebuilder"/>
		<rdfs:subClassOf rdf:resource="&java;JavaAPIPart"/>
		<rdfs:seeAlso rdf:resource="&android-1_6;JunitFramework"/>
		<rdfs:seeAlso rdf:resource="&android-1_6;JavaLang"/>
		<rdfs:seeAlso rdf:resource="&android-1_6;JavaUtil"/>
		<rdfs:seeAlso rdf:resource="&android-1_6;JavaLangAnnotation"/>
		<rdfs:seeAlso rdf:resource="&android-1_6;JavaLangReflect"/>
		<rdfs:comment xml:lang="en">Java API part implementing the android.test.suitebuilder package for Android 1.6</rdfs:comment>
	</owl:Class>
	<owl:Class rdf:about="&android-1_6;AndroidTestSuitebuilderAnnotation">
		<owl:equivalentClass rdf:resource="&android-1_5;AndroidTestSuitebuilderAnnotation"/>
		<rdfs:subClassOf rdf:resource="&java;JavaAPIPart"/>
		<rdfs:seeAlso rdf:resource="&android-1_6;JavaLangAnnotation"/>
		<rdfs:comment xml:lang="en">Java API part implementing the android.test.suitebuilder.annotation package for Android 1.6</rdfs:comment>
	</owl:Class>
	<owl:Class rdf:about="&android-1_6;JavaLang">
		<owl:equivalentClass rdf:resource="&android-1_5;JavaLang"/>
		<rdfs:subClassOf rdf:resource="&j2se-5_0;JavaLang"/>
		<rdfs:seeAlso rdf:resource="&android-1_6;JavaNio"/>
		<rdfs:seeAlso rdf:resource="&android-1_6;JavaSecurity"/>
		<rdfs:seeAlso rdf:resource="&android-1_6;JavaNet"/>
		<rdfs:seeAlso rdf:resource="&android-1_6;JavaUtil"/>
		<rdfs:seeAlso rdf:resource="&android-1_6;JavaIo"/>
		<rdfs:seeAlso rdf:resource="&android-1_6;JavaLangReflect"/>
		<rdfs:seeAlso rdf:resource="&android-1_6;JavaNioChannels"/>
		<rdfs:seeAlso rdf:resource="&android-1_6;JavaLangAnnotation"/>
		<rdfs:comment xml:lang="en">Java API part implementing the java.lang package for Android 1.6</rdfs:comment>
	</owl:Class>
	<owl:Class rdf:about="&android-1_6;JavaLangAnnotation">
		<owl:equivalentClass rdf:resource="&j2se-5_0;JavaLangAnnotation"/>
		<owl:equivalentClass rdf:resource="&android-1_5;JavaLangAnnotation"/>
		<rdfs:subClassOf rdf:resource="&java;JavaAPIPart"/>
		<rdfs:seeAlso rdf:resource="&android-1_6;JavaLang"/>
		<rdfs:seeAlso rdf:resource="&android-1_6;JavaLangReflect"/>
		<rdfs:comment xml:lang="en">Java API part implementing the java.lang.annotation package for Android 1.6</rdfs:comment>
	</owl:Class>
	<owl:Class rdf:about="&android-1_6;JavaLangReflect">
		<owl:equivalentClass rdf:resource="&j2se-5_0;JavaLangReflect"/>
		<owl:equivalentClass rdf:resource="&android-1_5;JavaLangReflect"/>
		<rdfs:subClassOf rdf:resource="&java;JavaAPIPart"/>
		<rdfs:seeAlso rdf:resource="&android-1_6;JavaLang"/>
		<rdfs:seeAlso rdf:resource="&android-1_6;JavaIo"/>
		<rdfs:seeAlso rdf:resource="&android-1_6;JavaSecurity"/>
		<rdfs:seeAlso rdf:resource="&android-1_6;JavaLangAnnotation"/>
		<rdfs:comment xml:lang="en">Java API part implementing the java.lang.reflect package for Android 1.6</rdfs:comment>
	</owl:Class>
	<owl:Class rdf:about="&android-1_6;JavaLangRef">
		<owl:equivalentClass rdf:resource="&j2se-5_0;JavaLangRef"/>
		<owl:equivalentClass rdf:resource="&android-1_5;JavaLangRef"/>
		<rdfs:subClassOf rdf:resource="&java;JavaAPIPart"/>
		<rdfs:seeAlso rdf:resource="&android-1_6;JavaLang"/>
		<rdfs:comment xml:lang="en">Java API part implementing the java.lang.ref package for Android 1.6</rdfs:comment>
	</owl:Class>
	<owl:Class rdf:about="&android-1_6;JavaUtil">
		<owl:equivalentClass rdf:resource="&j2se-5_0;JavaUtil"/>
		<owl:equivalentClass rdf:resource="&android-1_5;JavaUtil"/>
		<rdfs:subClassOf rdf:resource="&java;JavaAPIPart"/>
		<rdfs:seeAlso rdf:resource="&android-1_6;JavaUtilRegex"/>
		<rdfs:seeAlso rdf:resource="&android-1_6;JavaSecurity"/>
		<rdfs:seeAlso rdf:resource="&android-1_6;JavaIo"/>
		<rdfs:seeAlso rdf:resource="&android-1_6;JavaLang"/>
		<rdfs:seeAlso rdf:resource="&android-1_6;JavaNioChannels"/>
		<rdfs:seeAlso rdf:resource="&android-1_6;JavaMath"/>
		<rdfs:comment xml:lang="en">Java API part implementing the java.util package for Android 1.6</rdfs:comment>
	</owl:Class>
	<owl:Class rdf:about="&android-1_6;JavaUtilConcurrent">
		<owl:equivalentClass rdf:resource="&j2se-5_0;JavaUtilConcurrent"/>
		<owl:equivalentClass rdf:resource="&android-1_5;JavaUtilConcurrent"/>
		<rdfs:subClassOf rdf:resource="&java;JavaAPIPart"/>
		<rdfs:seeAlso rdf:resource="&android-1_6;JavaSecurity"/>
		<rdfs:seeAlso rdf:resource="&android-1_6;JavaUtil"/>
		<rdfs:seeAlso rdf:resource="&android-1_6;JavaIo"/>
		<rdfs:seeAlso rdf:resource="&android-1_6;JavaLang"/>
		<rdfs:comment xml:lang="en">Java API part implementing the java.util.concurrent package for Android 1.6</rdfs:comment>
	</owl:Class>
	<owl:Class rdf:about="&android-1_6;JavaUtilConcurrentAtomic">
		<owl:equivalentClass rdf:resource="&j2se-5_0;JavaUtilConcurrentAtomic"/>
		<owl:equivalentClass rdf:resource="&android-1_5;JavaUtilConcurrentAtomic"/>
		<rdfs:subClassOf rdf:resource="&java;JavaAPIPart"/>
		<rdfs:seeAlso rdf:resource="&android-1_6;JavaLang"/>
		<rdfs:seeAlso rdf:resource="&android-1_6;JavaIo"/>
		<rdfs:comment xml:lang="en">Java API part implementing the java.util.concurrent.atomic package for Android 1.6</rdfs:comment>
	</owl:Class>
	<owl:Class rdf:about="&android-1_6;JavaUtilConcurrentLocks">
		<owl:equivalentClass rdf:resource="&j2se-5_0;JavaUtilConcurrentLocks"/>
		<owl:equivalentClass rdf:resource="&android-1_5;JavaUtilConcurrentLocks"/>
		<rdfs:subClassOf rdf:resource="&java;JavaAPIPart"/>
		<rdfs:seeAlso rdf:resource="&android-1_6;JavaLang"/>
		<rdfs:seeAlso rdf:resource="&android-1_6;JavaUtilConcurrent"/>
		<rdfs:seeAlso rdf:resource="&android-1_6;JavaUtil"/>
		<rdfs:seeAlso rdf:resource="&android-1_6;JavaIo"/>
		<rdfs:comment xml:lang="en">Java API part implementing the java.util.concurrent.locks package for Android 1.6</rdfs:comment>
	</owl:Class>
	<owl:Class rdf:about="&android-1_6;JavaUtilRegex">
		<owl:equivalentClass rdf:resource="&j2se-5_0;JavaUtilRegex"/>
		<owl:equivalentClass rdf:resource="&android-1_5;JavaUtilRegex"/>
		<rdfs:subClassOf rdf:resource="&java;JavaAPIPart"/>
		<rdfs:seeAlso rdf:resource="&android-1_6;JavaLang"/>
		<rdfs:seeAlso rdf:resource="&android-1_6;JavaIo"/>
		<rdfs:comment xml:lang="en">Java API part implementing the java.util.regex package for Android 1.6</rdfs:comment>
	</owl:Class>
	<owl:Class rdf:about="&android-1_6;JavaUtilJar">
		<owl:equivalentClass rdf:resource="&j2se-5_0;JavaUtilJar"/>
		<owl:equivalentClass rdf:resource="&android-1_5;JavaUtilJar"/>
		<rdfs:subClassOf rdf:resource="&java;JavaAPIPart"/>
		<rdfs:seeAlso rdf:resource="&android-1_6;JavaLang"/>
		<rdfs:seeAlso rdf:resource="&android-1_6;JavaBeans"/>
		<rdfs:seeAlso rdf:resource="&android-1_6;JavaUtilZip"/>
		<rdfs:seeAlso rdf:resource="&android-1_6;JavaUtil"/>
		<rdfs:seeAlso rdf:resource="&android-1_6;JavaIo"/>
		<rdfs:comment xml:lang="en">Java API part implementing the java.util.jar package for Android 1.6</rdfs:comment>
	</owl:Class>
	<owl:Class rdf:about="&android-1_6;JavaUtilZip">
		<owl:equivalentClass rdf:resource="&j2se-5_0;JavaUtilZip"/>
		<owl:equivalentClass rdf:resource="&android-1_5;JavaUtilZip"/>
		<rdfs:subClassOf rdf:resource="&java;JavaAPIPart"/>
		<rdfs:seeAlso rdf:resource="&android-1_6;JavaLang"/>
		<rdfs:seeAlso rdf:resource="&android-1_6;JavaUtil"/>
		<rdfs:seeAlso rdf:resource="&android-1_6;JavaIo"/>
		<rdfs:comment xml:lang="en">Java API part implementing the java.util.zip package for Android 1.6</rdfs:comment>
	</owl:Class>
	<owl:Class rdf:about="&android-1_6;JavaUtilLogging">
		<owl:equivalentClass rdf:resource="&j2se-5_0;JavaUtilLogging"/>
		<owl:equivalentClass rdf:resource="&android-1_5;JavaUtilLogging"/>
		<rdfs:subClassOf rdf:resource="&java;JavaAPIPart"/>
		<rdfs:seeAlso rdf:resource="&android-1_6;JavaLang"/>
		<rdfs:seeAlso rdf:resource="&android-1_6;JavaSecurity"/>
		<rdfs:seeAlso rdf:resource="&android-1_6;JavaBeans"/>
		<rdfs:seeAlso rdf:resource="&android-1_6;JavaUtil"/>
		<rdfs:seeAlso rdf:resource="&android-1_6;JavaIo"/>
		<rdfs:comment xml:lang="en">Java API part implementing the java.util.logging package for Android 1.6</rdfs:comment>
	</owl:Class>
	<owl:Class rdf:about="&android-1_6;JavaUtilPrefs">
		<owl:equivalentClass rdf:resource="&j2se-5_0;JavaUtilPrefs"/>
		<owl:equivalentClass rdf:resource="&android-1_5;JavaUtilPrefs"/>
		<rdfs:subClassOf rdf:resource="&java;JavaAPIPart"/>
		<rdfs:seeAlso rdf:resource="&android-1_6;JavaLang"/>
		<rdfs:seeAlso rdf:resource="&android-1_6;JavaUtil"/>
		<rdfs:seeAlso rdf:resource="&android-1_6;JavaIo"/>
		<rdfs:comment xml:lang="en">Java API part implementing the java.util.prefs package for Android 1.6</rdfs:comment>
	</owl:Class>
	<owl:Class rdf:about="&android-1_6;JavaIo">
		<owl:equivalentClass rdf:resource="&j2se-5_0;JavaIo"/>
		<owl:equivalentClass rdf:resource="&android-1_5;JavaIo"/>
		<rdfs:subClassOf rdf:resource="&java;JavaAPIPart"/>
		<rdfs:seeAlso rdf:resource="&android-1_6;JavaNio"/>
		<rdfs:seeAlso rdf:resource="&android-1_6;JavaLang"/>
		<rdfs:seeAlso rdf:resource="&android-1_6;JavaNioChannels"/>
		<rdfs:seeAlso rdf:resource="&android-1_6;JavaSecurity"/>
		<rdfs:seeAlso rdf:resource="&android-1_6;JavaNet"/>
		<rdfs:seeAlso rdf:resource="&android-1_6;JavaNioCharset"/>
		<rdfs:seeAlso rdf:resource="&android-1_6;JavaUtil"/>
		<rdfs:comment xml:lang="en">Java API part implementing the java.io package for Android 1.6</rdfs:comment>
	</owl:Class>
	<owl:Class rdf:about="&android-1_6;JavaNio">
		<owl:equivalentClass rdf:resource="&j2se-5_0;JavaNio"/>
		<owl:equivalentClass rdf:resource="&android-1_5;JavaNio"/>
		<rdfs:subClassOf rdf:resource="&java;JavaAPIPart"/>
		<rdfs:seeAlso rdf:resource="&android-1_6;JavaLang"/>
		<rdfs:comment xml:lang="en">Java API part implementing the java.nio package for Android 1.6</rdfs:comment>
	</owl:Class>
	<owl:Class rdf:about="&android-1_6;JavaNioChannels">
		<owl:equivalentClass rdf:resource="&j2se-5_0;JavaNioChannels"/>
		<owl:equivalentClass rdf:resource="&android-1_5;JavaNioChannels"/>
		<rdfs:subClassOf rdf:resource="&java;JavaAPIPart"/>
		<rdfs:seeAlso rdf:resource="&android-1_6;JavaNio"/>
		<rdfs:seeAlso rdf:resource="&android-1_6;JavaNioChannelsSpi"/>
		<rdfs:seeAlso rdf:resource="&android-1_6;JavaLang"/>
		<rdfs:seeAlso rdf:resource="&android-1_6;JavaNet"/>
		<rdfs:seeAlso rdf:resource="&android-1_6;JavaNioCharset"/>
		<rdfs:seeAlso rdf:resource="&android-1_6;JavaUtil"/>
		<rdfs:seeAlso rdf:resource="&android-1_6;JavaIo"/>
		<rdfs:comment xml:lang="en">Java API part implementing the java.nio.channels package for Android 1.6</rdfs:comment>
	</owl:Class>
	<owl:Class rdf:about="&android-1_6;JavaNioChannelsSpi">
		<owl:equivalentClass rdf:resource="&j2se-5_0;JavaNioChannelsSpi"/>
		<owl:equivalentClass rdf:resource="&android-1_5;JavaNioChannelsSpi"/>
		<rdfs:subClassOf rdf:resource="&java;JavaAPIPart"/>
		<rdfs:seeAlso rdf:resource="&android-1_6;JavaLang"/>
		<rdfs:seeAlso rdf:resource="&android-1_6;JavaNioChannels"/>
		<rdfs:seeAlso rdf:resource="&android-1_6;JavaUtil"/>
		<rdfs:comment xml:lang="en">Java API part implementing the java.nio.channels.spi package for Android 1.6</rdfs:comment>
	</owl:Class>
	<owl:Class rdf:about="&android-1_6;JavaNioCharset">
		<owl:equivalentClass rdf:resource="&j2se-5_0;JavaNioCharset"/>
		<owl:equivalentClass rdf:resource="&android-1_5;JavaNioCharset"/>
		<rdfs:subClassOf rdf:resource="&java;JavaAPIPart"/>
		<rdfs:seeAlso rdf:resource="&android-1_6;JavaNio"/>
		<rdfs:seeAlso rdf:resource="&android-1_6;JavaLang"/>
		<rdfs:seeAlso rdf:resource="&android-1_6;JavaUtil"/>
		<rdfs:seeAlso rdf:resource="&android-1_6;JavaIo"/>
		<rdfs:comment xml:lang="en">Java API part implementing the java.nio.charset package for Android 1.6</rdfs:comment>
	</owl:Class>
	<owl:Class rdf:about="&android-1_6;JavaNioCharsetSpi">
		<owl:equivalentClass rdf:resource="&j2se-5_0;JavaNioCharsetSpi"/>
		<owl:equivalentClass rdf:resource="&android-1_5;JavaNioCharsetSpi"/>
		<rdfs:subClassOf rdf:resource="&java;JavaAPIPart"/>
		<rdfs:seeAlso rdf:resource="&android-1_6;JavaLang"/>
		<rdfs:seeAlso rdf:resource="&android-1_6;JavaUtil"/>
		<rdfs:seeAlso rdf:resource="&android-1_6;JavaNioCharset"/>
		<rdfs:comment xml:lang="en">Java API part implementing the java.nio.charset.spi package for Android 1.6</rdfs:comment>
	</owl:Class>
	<owl:Class rdf:about="&android-1_6;JavaNet">
		<owl:equivalentClass rdf:resource="&j2se-5_0;JavaNet"/>
		<owl:equivalentClass rdf:resource="&android-1_5;JavaNet"/>
		<rdfs:subClassOf rdf:resource="&java;JavaAPIPart"/>
		<rdfs:seeAlso rdf:resource="&android-1_6;JavaSecurity"/>
		<rdfs:seeAlso rdf:resource="&android-1_6;JavaUtilJar"/>
		<rdfs:seeAlso rdf:resource="&android-1_6;JavaUtil"/>
		<rdfs:seeAlso rdf:resource="&android-1_6;JavaIo"/>
		<rdfs:seeAlso rdf:resource="&android-1_6;JavaLang"/>
		<rdfs:seeAlso rdf:resource="&android-1_6;JavaNioChannels"/>
		<rdfs:comment xml:lang="en">Java API part implementing the java.net package for Android 1.6</rdfs:comment>
	</owl:Class>
	<owl:Class rdf:about="&android-1_6;JavaSecurity">
		<owl:equivalentClass rdf:resource="&j2se-5_0;JavaSecurity"/>
		<owl:equivalentClass rdf:resource="&android-1_5;JavaSecurity"/>
		<rdfs:subClassOf rdf:resource="&java;JavaAPIPart"/>
		<rdfs:seeAlso rdf:resource="&android-1_6;JavaNio"/>
		<rdfs:seeAlso rdf:resource="&android-1_6;JavaxSecurityAuth"/>
		<rdfs:seeAlso rdf:resource="&android-1_6;JavaNet"/>
		<rdfs:seeAlso rdf:resource="&android-1_6;JavaSecurityCert"/>
		<rdfs:seeAlso rdf:resource="&android-1_6;JavaxCrypto"/>
		<rdfs:seeAlso rdf:resource="&android-1_6;JavaUtil"/>
		<rdfs:seeAlso rdf:resource="&android-1_6;JavaIo"/>
		<rdfs:seeAlso rdf:resource="&android-1_6;JavaxSecurityAuthCallback"/>
		<rdfs:seeAlso rdf:resource="&android-1_6;JavaLang"/>
		<rdfs:seeAlso rdf:resource="&android-1_6;JavaSecuritySpec"/>
		<rdfs:comment xml:lang="en">Java API part implementing the java.security package for Android 1.6</rdfs:comment>
	</owl:Class>
	<owl:Class rdf:about="&android-1_6;JavaSecurityCert">
		<owl:equivalentClass rdf:resource="&j2se-5_0;JavaSecurityCert"/>
		<owl:equivalentClass rdf:resource="&android-1_5;JavaSecurityCert"/>
		<rdfs:subClassOf rdf:resource="&java;JavaAPIPart"/>
		<rdfs:seeAlso rdf:resource="&android-1_6;JavaLang"/>
		<rdfs:seeAlso rdf:resource="&android-1_6;JavaSecurity"/>
		<rdfs:seeAlso rdf:resource="&android-1_6;JavaMath"/>
		<rdfs:seeAlso rdf:resource="&android-1_6;JavaxSecurityAuthX500"/>
		<rdfs:seeAlso rdf:resource="&android-1_6;JavaUtil"/>
		<rdfs:seeAlso rdf:resource="&android-1_6;JavaIo"/>
		<rdfs:comment xml:lang="en">Java API part implementing the java.security.cert package for Android 1.6</rdfs:comment>
	</owl:Class>
	<owl:Class rdf:about="&android-1_6;JavaSecuritySpec">
		<owl:equivalentClass rdf:resource="&j2se-5_0;JavaSecuritySpec"/>
		<owl:equivalentClass rdf:resource="&android-1_5;JavaSecuritySpec"/>
		<rdfs:subClassOf rdf:resource="&java;JavaAPIPart"/>
		<rdfs:seeAlso rdf:resource="&android-1_6;JavaLang"/>
		<rdfs:seeAlso rdf:resource="&android-1_6;JavaSecurityInterfaces"/>
		<rdfs:seeAlso rdf:resource="&android-1_6;JavaSecurity"/>
		<rdfs:seeAlso rdf:resource="&android-1_6;JavaMath"/>
		<rdfs:comment xml:lang="en">Java API part implementing the java.security.spec package for Android 1.6</rdfs:comment>
	</owl:Class>
	<owl:Class rdf:about="&android-1_6;JavaSecurityAcl">
		<owl:equivalentClass rdf:resource="&j2se-5_0;JavaSecurityAcl"/>
		<owl:equivalentClass rdf:resource="&android-1_5;JavaSecurityAcl"/>
		<rdfs:subClassOf rdf:resource="&java;JavaAPIPart"/>
		<rdfs:seeAlso rdf:resource="&android-1_6;JavaLang"/>
		<rdfs:seeAlso rdf:resource="&android-1_6;JavaUtil"/>
		<rdfs:seeAlso rdf:resource="&android-1_6;JavaSecurity"/>
		<rdfs:comment xml:lang="en">Java API part implementing the java.security.acl package for Android 1.6</rdfs:comment>
	</owl:Class>
	<owl:Class rdf:about="&android-1_6;JavaSecurityInterfaces">
		<owl:equivalentClass rdf:resource="&j2se-5_0;JavaSecurityInterfaces"/>
		<owl:equivalentClass rdf:resource="&android-1_5;JavaSecurityInterfaces"/>
		<rdfs:subClassOf rdf:resource="&java;JavaAPIPart"/>
		<rdfs:seeAlso rdf:resource="&android-1_6;JavaSecuritySpec"/>
		<rdfs:seeAlso rdf:resource="&android-1_6;JavaSecurity"/>
		<rdfs:seeAlso rdf:resource="&android-1_6;JavaMath"/>
		<rdfs:comment xml:lang="en">Java API part implementing the java.security.interfaces package for Android 1.6</rdfs:comment>
	</owl:Class>
	<owl:Class rdf:about="&android-1_6;JavaText">
		<owl:equivalentClass rdf:resource="&j2se-5_0;JavaText"/>
		<owl:equivalentClass rdf:resource="&android-1_5;JavaText"/>
		<rdfs:subClassOf rdf:resource="&java;JavaAPIPart"/>
		<rdfs:seeAlso rdf:resource="&android-1_6;JavaLang"/>
		<rdfs:seeAlso rdf:resource="&android-1_6;JavaUtil"/>
		<rdfs:seeAlso rdf:resource="&android-1_6;JavaIo"/>
		<rdfs:comment xml:lang="en">Java API part implementing the java.text package for Android 1.6</rdfs:comment>
	</owl:Class>
	<owl:Class rdf:about="&android-1_6;JavaAwtFont">
		<owl:equivalentClass rdf:resource="&android-1_5;JavaAwtFont"/>
		<rdfs:subClassOf rdf:resource="&java;JavaAPIPart"/>
		<rdfs:seeAlso rdf:resource="&android-1_6;JavaLang"/>
		<rdfs:seeAlso rdf:resource="&android-1_6;JavaText"/>
		<rdfs:seeAlso rdf:resource="&android-1_6;JavaIo"/>
		<rdfs:comment xml:lang="en">Java API part implementing the java.awt.font package for Android 1.6</rdfs:comment>
	</owl:Class>
	<owl:Class rdf:about="&android-1_6;JavaBeans">
		<owl:equivalentClass rdf:resource="&android-1_5;JavaBeans"/>
		<rdfs:subClassOf rdf:resource="&java;JavaAPIPart"/>
		<rdfs:seeAlso rdf:resource="&android-1_6;JavaLang"/>
		<rdfs:seeAlso rdf:resource="&android-1_6;JavaUtil"/>
		<rdfs:seeAlso rdf:resource="&android-1_6;JavaIo"/>
		<rdfs:comment xml:lang="en">Java API part implementing the java.beans package for Android 1.6</rdfs:comment>
	</owl:Class>
	<owl:Class rdf:about="&android-1_6;JavaMath">
		<owl:equivalentClass rdf:resource="&j2se-5_0;JavaMath"/>
		<owl:equivalentClass rdf:resource="&android-1_5;JavaMath"/>
		<rdfs:subClassOf rdf:resource="&java;JavaAPIPart"/>
		<rdfs:seeAlso rdf:resource="&android-1_6;JavaLang"/>
		<rdfs:seeAlso rdf:resource="&android-1_6;JavaUtil"/>
		<rdfs:seeAlso rdf:resource="&android-1_6;JavaIo"/>
		<rdfs:comment xml:lang="en">Java API part implementing the java.math package for Android 1.6</rdfs:comment>
	</owl:Class>
	<owl:Class rdf:about="&android-1_6;JavaSql">
		<owl:equivalentClass rdf:resource="&j2se-5_0;JavaSql"/>
		<owl:equivalentClass rdf:resource="&android-1_5;JavaSql"/>
		<rdfs:subClassOf rdf:resource="&java;JavaAPIPart"/>
		<rdfs:seeAlso rdf:resource="&android-1_6;JavaLang"/>
		<rdfs:seeAlso rdf:resource="&android-1_6;JavaSecurity"/>
		<rdfs:seeAlso rdf:resource="&android-1_6;JavaNet"/>
		<rdfs:seeAlso rdf:resource="&android-1_6;JavaMath"/>
		<rdfs:seeAlso rdf:resource="&android-1_6;JavaUtil"/>
		<rdfs:seeAlso rdf:resource="&android-1_6;JavaIo"/>
		<rdfs:comment xml:lang="en">Java API part implementing the java.sql package for Android 1.6</rdfs:comment>
	</owl:Class>
	<owl:Class rdf:about="&android-1_6;OrgXmlpullV1">
		<owl:equivalentClass rdf:resource="&android-1_5;OrgXmlpullV1"/>
		<rdfs:subClassOf rdf:resource="&java;JavaAPIPart"/>
		<rdfs:seeAlso rdf:resource="&android-1_6;JavaLang"/>
		<rdfs:seeAlso rdf:resource="&android-1_6;JavaUtil"/>
		<rdfs:seeAlso rdf:resource="&android-1_6;JavaIo"/>
		<rdfs:comment xml:lang="en">Java API part implementing the org.xmlpull.v1 package for Android 1.6</rdfs:comment>
	</owl:Class>
	<owl:Class rdf:about="&android-1_6;OrgXmlpullV1Sax2">
		<owl:equivalentClass rdf:resource="&android-1_5;OrgXmlpullV1Sax2"/>
		<rdfs:subClassOf rdf:resource="&java;JavaAPIPart"/>
		<rdfs:seeAlso rdf:resource="&android-1_6;JavaLang"/>
		<rdfs:seeAlso rdf:resource="&android-1_6;OrgXmlSax"/>
		<rdfs:seeAlso rdf:resource="&android-1_6;OrgXmlpullV1"/>
		<rdfs:comment xml:lang="en">Java API part implementing the org.xmlpull.v1.sax2 package for Android 1.6</rdfs:comment>
	</owl:Class>
	<owl:Class rdf:about="&android-1_6;OrgXmlSax">
		<owl:equivalentClass rdf:resource="&j2se-5_0;OrgXmlSax"/>
		<owl:equivalentClass rdf:resource="&android-1_5;OrgXmlSax"/>
		<rdfs:subClassOf rdf:resource="&java;JavaAPIPart"/>
		<rdfs:seeAlso rdf:resource="&android-1_6;JavaLang"/>
		<rdfs:seeAlso rdf:resource="&android-1_6;JavaUtil"/>
		<rdfs:seeAlso rdf:resource="&android-1_6;JavaIo"/>
		<rdfs:comment xml:lang="en">Java API part implementing the org.xml.sax package for Android 1.6</rdfs:comment>
	</owl:Class>
	<owl:Class rdf:about="&android-1_6;OrgXmlSaxHelpers">
		<owl:equivalentClass rdf:resource="&j2se-5_0;OrgXmlSaxHelpers"/>
		<owl:equivalentClass rdf:resource="&android-1_5;OrgXmlSaxHelpers"/>
		<rdfs:subClassOf rdf:resource="&java;JavaAPIPart"/>
		<rdfs:seeAlso rdf:resource="&android-1_6;JavaLang"/>
		<rdfs:seeAlso rdf:resource="&android-1_6;JavaUtil"/>
		<rdfs:seeAlso rdf:resource="&android-1_6;OrgXmlSax"/>
		<rdfs:comment xml:lang="en">Java API part implementing the org.xml.sax.helpers package for Android 1.6</rdfs:comment>
	</owl:Class>
	<owl:Class rdf:about="&android-1_6;OrgXmlSaxExt">
		<owl:equivalentClass rdf:resource="&j2se-5_0;OrgXmlSaxExt"/>
		<owl:equivalentClass rdf:resource="&android-1_5;OrgXmlSaxExt"/>
		<rdfs:subClassOf rdf:resource="&java;JavaAPIPart"/>
		<rdfs:seeAlso rdf:resource="&android-1_6;JavaLang"/>
		<rdfs:seeAlso rdf:resource="&android-1_6;OrgXmlSax"/>
		<rdfs:seeAlso rdf:resource="&android-1_6;OrgXmlSaxHelpers"/>
		<rdfs:comment xml:lang="en">Java API part implementing the org.xml.sax.ext package for Android 1.6</rdfs:comment>
	</owl:Class>
	<owl:Class rdf:about="&android-1_6;OrgW3cDom">
		<owl:equivalentClass rdf:resource="&android-1_5;OrgW3cDom"/>
		<rdfs:subClassOf rdf:resource="&java;JavaAPIPart"/>
		<rdfs:seeAlso rdf:resource="&android-1_6;JavaLang"/>
		<rdfs:comment xml:lang="en">Java API part implementing the org.w3c.dom package for Android 1.6</rdfs:comment>
	</owl:Class>
	<owl:Class rdf:about="&android-1_6;OrgApacheCommonsLogging">
		<owl:equivalentClass rdf:resource="&android-1_5;OrgApacheCommonsLogging"/>
		<rdfs:subClassOf rdf:resource="&java;JavaAPIPart"/>
		<rdfs:seeAlso rdf:resource="&android-1_6;JavaLang"/>
		<rdfs:comment xml:lang="en">Java API part implementing the org.apache.commons.logging package for Android 1.6</rdfs:comment>
	</owl:Class>
	<owl:Class rdf:about="&android-1_6;OrgApacheHttp">
		<owl:equivalentClass rdf:resource="&android-1_5;OrgApacheHttp"/>
		<rdfs:subClassOf rdf:resource="&java;JavaAPIPart"/>
		<rdfs:seeAlso rdf:resource="&android-1_6;JavaLang"/>
		<rdfs:seeAlso rdf:resource="&android-1_6;OrgApacheHttpUtil"/>
		<rdfs:seeAlso rdf:resource="&android-1_6;OrgApacheHttpProtocol"/>
		<rdfs:seeAlso rdf:resource="&android-1_6;JavaNet"/>
		<rdfs:seeAlso rdf:resource="&android-1_6;OrgApacheHttpParams"/>
		<rdfs:seeAlso rdf:resource="&android-1_6;JavaUtil"/>
		<rdfs:seeAlso rdf:resource="&android-1_6;JavaIo"/>
		<rdfs:comment xml:lang="en">Java API part implementing the org.apache.http package for Android 1.6</rdfs:comment>
	</owl:Class>
	<owl:Class rdf:about="&android-1_6;OrgApacheHttpProtocol">
		<owl:equivalentClass rdf:resource="&android-1_5;OrgApacheHttpProtocol"/>
		<rdfs:subClassOf rdf:resource="&java;JavaAPIPart"/>
		<rdfs:seeAlso rdf:resource="&android-1_6;JavaLang"/>
		<rdfs:seeAlso rdf:resource="&android-1_6;OrgApacheHttp"/>
		<rdfs:seeAlso rdf:resource="&android-1_6;OrgApacheHttpParams"/>
		<rdfs:seeAlso rdf:resource="&android-1_6;JavaUtil"/>
		<rdfs:comment xml:lang="en">Java API part implementing the org.apache.http.protocol package for Android 1.6</rdfs:comment>
	</owl:Class>
	<owl:Class rdf:about="&android-1_6;OrgApacheHttpUtil">
		<owl:equivalentClass rdf:resource="&android-1_5;OrgApacheHttpUtil"/>
		<rdfs:subClassOf rdf:resource="&java;JavaAPIPart"/>
		<rdfs:seeAlso rdf:resource="&android-1_6;JavaLang"/>
		<rdfs:seeAlso rdf:resource="&android-1_6;OrgApacheHttp"/>
		<rdfs:seeAlso rdf:resource="&android-1_6;JavaUtil"/>
		<rdfs:comment xml:lang="en">Java API part implementing the org.apache.http.util package for Android 1.6</rdfs:comment>
	</owl:Class>
	<owl:Class rdf:about="&android-1_6;OrgApacheHttpParams">
		<owl:equivalentClass rdf:resource="&android-1_5;OrgApacheHttpParams"/>
		<rdfs:subClassOf rdf:resource="&java;JavaAPIPart"/>
		<rdfs:seeAlso rdf:resource="&android-1_6;JavaLang"/>
		<rdfs:seeAlso rdf:resource="&android-1_6;OrgApacheHttp"/>
		<rdfs:seeAlso rdf:resource="&android-1_6;JavaIo"/>
		<rdfs:comment xml:lang="en">Java API part implementing the org.apache.http.params package for Android 1.6</rdfs:comment>
	</owl:Class>
	<owl:Class rdf:about="&android-1_6;OrgApacheHttpAuth">
		<owl:equivalentClass rdf:resource="&android-1_5;OrgApacheHttpAuth"/>
		<rdfs:subClassOf rdf:resource="&java;JavaAPIPart"/>
		<rdfs:seeAlso rdf:resource="&android-1_6;JavaLang"/>
		<rdfs:seeAlso rdf:resource="&android-1_6;OrgApacheHttp"/>
		<rdfs:seeAlso rdf:resource="&android-1_6;JavaUtil"/>
		<rdfs:seeAlso rdf:resource="&android-1_6;JavaSecurity"/>
		<rdfs:seeAlso rdf:resource="&android-1_6;OrgApacheHttpParams"/>
		<rdfs:comment xml:lang="en">Java API part implementing the org.apache.http.auth package for Android 1.6</rdfs:comment>
	</owl:Class>
	<owl:Class rdf:about="&android-1_6;OrgApacheHttpAuthParams">
		<owl:equivalentClass rdf:resource="&android-1_5;OrgApacheHttpAuthParams"/>
		<rdfs:subClassOf rdf:resource="&java;JavaAPIPart"/>
		<rdfs:seeAlso rdf:resource="&android-1_6;JavaLang"/>
		<rdfs:seeAlso rdf:resource="&android-1_6;OrgApacheHttpParams"/>
		<rdfs:comment xml:lang="en">Java API part implementing the org.apache.http.auth.params package for Android 1.6</rdfs:comment>
	</owl:Class>
	<owl:Class rdf:about="&android-1_6;OrgApacheHttpClient">
		<owl:equivalentClass rdf:resource="&android-1_5;OrgApacheHttpClient"/>
		<rdfs:subClassOf rdf:resource="&java;JavaAPIPart"/>
		<rdfs:seeAlso rdf:resource="&android-1_6;OrgApacheHttpClientMethods"/>
		<rdfs:seeAlso rdf:resource="&android-1_6;JavaLang"/>
		<rdfs:seeAlso rdf:resource="&android-1_6;OrgApacheHttp"/>
		<rdfs:seeAlso rdf:resource="&android-1_6;OrgApacheHttpProtocol"/>
		<rdfs:seeAlso rdf:resource="&android-1_6;JavaNet"/>
		<rdfs:seeAlso rdf:resource="&android-1_6;OrgApacheHttpParams"/>
		<rdfs:seeAlso rdf:resource="&android-1_6;OrgApacheHttpAuth"/>
		<rdfs:seeAlso rdf:resource="&android-1_6;OrgApacheHttpCookie"/>
		<rdfs:seeAlso rdf:resource="&android-1_6;JavaUtil"/>
		<rdfs:seeAlso rdf:resource="&android-1_6;JavaIo"/>
		<rdfs:seeAlso rdf:resource="&android-1_6;OrgApacheHttpConn"/>
		<rdfs:comment xml:lang="en">Java API part implementing the org.apache.http.client package for Android 1.6</rdfs:comment>
	</owl:Class>
	<owl:Class rdf:about="&android-1_6;OrgApacheHttpClientMethods">
		<owl:equivalentClass rdf:resource="&android-1_5;OrgApacheHttpClientMethods"/>
		<rdfs:subClassOf rdf:resource="&java;JavaAPIPart"/>
		<rdfs:seeAlso rdf:resource="&android-1_6;JavaLang"/>
		<rdfs:seeAlso rdf:resource="&android-1_6;OrgApacheHttp"/>
		<rdfs:seeAlso rdf:resource="&android-1_6;JavaNet"/>
		<rdfs:seeAlso rdf:resource="&android-1_6;OrgApacheHttpMessage"/>
		<rdfs:seeAlso rdf:resource="&android-1_6;JavaUtil"/>
		<rdfs:seeAlso rdf:resource="&android-1_6;OrgApacheHttpConn"/>
		<rdfs:comment xml:lang="en">Java API part implementing the org.apache.http.client.methods package for Android 1.6</rdfs:comment>
	</owl:Class>
	<owl:Class rdf:about="&android-1_6;OrgApacheHttpClientEntity">
		<owl:equivalentClass rdf:resource="&android-1_5;OrgApacheHttpClientEntity"/>
		<rdfs:subClassOf rdf:resource="&java;JavaAPIPart"/>
		<rdfs:seeAlso rdf:resource="&android-1_6;JavaLang"/>
		<rdfs:seeAlso rdf:resource="&android-1_6;OrgApacheHttpEntity"/>
		<rdfs:seeAlso rdf:resource="&android-1_6;JavaUtil"/>
		<rdfs:comment xml:lang="en">Java API part implementing the org.apache.http.client.entity package for Android 1.6</rdfs:comment>
	</owl:Class>
	<owl:Class rdf:about="&android-1_6;OrgApacheHttpClientParams">
		<owl:equivalentClass rdf:resource="&android-1_5;OrgApacheHttpClientParams"/>
		<rdfs:subClassOf rdf:resource="&java;JavaAPIPart"/>
		<rdfs:seeAlso rdf:resource="&android-1_6;JavaLang"/>
		<rdfs:seeAlso rdf:resource="&android-1_6;OrgApacheHttp"/>
		<rdfs:seeAlso rdf:resource="&android-1_6;OrgApacheHttpAuthParams"/>
		<rdfs:seeAlso rdf:resource="&android-1_6;OrgApacheHttpParams"/>
		<rdfs:seeAlso rdf:resource="&android-1_6;OrgApacheHttpConnParams"/>
		<rdfs:seeAlso rdf:resource="&android-1_6;JavaUtil"/>
		<rdfs:seeAlso rdf:resource="&android-1_6;OrgApacheHttpCookieParams"/>
		<rdfs:seeAlso rdf:resource="&android-1_6;OrgApacheHttpConn"/>
		<rdfs:comment xml:lang="en">Java API part implementing the org.apache.http.client.params package for Android 1.6</rdfs:comment>
	</owl:Class>
	<owl:Class rdf:about="&android-1_6;OrgApacheHttpClientProtocol">
		<owl:equivalentClass rdf:resource="&android-1_5;OrgApacheHttpClientProtocol"/>
		<rdfs:subClassOf rdf:resource="&java;JavaAPIPart"/>
		<rdfs:seeAlso rdf:resource="&android-1_6;JavaLang"/>
		<rdfs:seeAlso rdf:resource="&android-1_6;OrgApacheHttp"/>
		<rdfs:seeAlso rdf:resource="&android-1_6;OrgApacheHttpProtocol"/>
		<rdfs:seeAlso rdf:resource="&android-1_6;OrgApacheHttpAuth"/>
		<rdfs:seeAlso rdf:resource="&android-1_6;OrgApacheHttpCookie"/>
		<rdfs:seeAlso rdf:resource="&android-1_6;JavaUtil"/>
		<rdfs:seeAlso rdf:resource="&android-1_6;OrgApacheHttpClient"/>
		<rdfs:comment xml:lang="en">Java API part implementing the org.apache.http.client.protocol package for Android 1.6</rdfs:comment>
	</owl:Class>
	<owl:Class rdf:about="&android-1_6;OrgApacheHttpClientUtils">
		<owl:equivalentClass rdf:resource="&android-1_5;OrgApacheHttpClientUtils"/>
		<rdfs:subClassOf rdf:resource="&java;JavaAPIPart"/>
		<rdfs:seeAlso rdf:resource="&android-1_6;JavaLang"/>
		<rdfs:seeAlso rdf:resource="&android-1_6;OrgApacheHttp"/>
		<rdfs:seeAlso rdf:resource="&android-1_6;JavaUtil"/>
		<rdfs:seeAlso rdf:resource="&android-1_6;JavaNet"/>
		<rdfs:comment xml:lang="en">Java API part implementing the org.apache.http.client.utils package for Android 1.6</rdfs:comment>
	</owl:Class>
	<owl:Class rdf:about="&android-1_6;OrgApacheHttpCookie">
		<owl:equivalentClass rdf:resource="&android-1_5;OrgApacheHttpCookie"/>
		<rdfs:subClassOf rdf:resource="&java;JavaAPIPart"/>
		<rdfs:seeAlso rdf:resource="&android-1_6;JavaLang"/>
		<rdfs:seeAlso rdf:resource="&android-1_6;OrgApacheHttp"/>
		<rdfs:seeAlso rdf:resource="&android-1_6;JavaUtil"/>
		<rdfs:seeAlso rdf:resource="&android-1_6;JavaIo"/>
		<rdfs:seeAlso rdf:resource="&android-1_6;OrgApacheHttpParams"/>
		<rdfs:comment xml:lang="en">Java API part implementing the org.apache.http.cookie package for Android 1.6</rdfs:comment>
	</owl:Class>
	<owl:Class rdf:about="&android-1_6;OrgApacheHttpCookieParams">
		<owl:equivalentClass rdf:resource="&android-1_5;OrgApacheHttpCookieParams"/>
		<rdfs:subClassOf rdf:resource="&java;JavaAPIPart"/>
		<rdfs:seeAlso rdf:resource="&android-1_6;JavaLang"/>
		<rdfs:seeAlso rdf:resource="&android-1_6;JavaUtil"/>
		<rdfs:seeAlso rdf:resource="&android-1_6;OrgApacheHttpParams"/>
		<rdfs:comment xml:lang="en">Java API part implementing the org.apache.http.cookie.params package for Android 1.6</rdfs:comment>
	</owl:Class>
	<owl:Class rdf:about="&android-1_6;OrgApacheHttpConn">
		<owl:equivalentClass rdf:resource="&android-1_5;OrgApacheHttpConn"/>
		<rdfs:subClassOf rdf:resource="&java;JavaAPIPart"/>
		<rdfs:seeAlso rdf:resource="&android-1_6;JavaLang"/>
		<rdfs:seeAlso rdf:resource="&android-1_6;OrgApacheHttpEntity"/>
		<rdfs:seeAlso rdf:resource="&android-1_6;OrgApacheHttp"/>
		<rdfs:seeAlso rdf:resource="&android-1_6;OrgApacheHttpProtocol"/>
		<rdfs:seeAlso rdf:resource="&android-1_6;JavaxNetSsl"/>
		<rdfs:seeAlso rdf:resource="&android-1_6;JavaNet"/>
		<rdfs:seeAlso rdf:resource="&android-1_6;OrgApacheHttpConnRouting"/>
		<rdfs:seeAlso rdf:resource="&android-1_6;OrgApacheHttpConnScheme"/>
		<rdfs:seeAlso rdf:resource="&android-1_6;OrgApacheHttpParams"/>
		<rdfs:seeAlso rdf:resource="&android-1_6;JavaUtilConcurrent"/>
		<rdfs:seeAlso rdf:resource="&android-1_6;JavaIo"/>
		<rdfs:comment xml:lang="en">Java API part implementing the org.apache.http.conn package for Android 1.6</rdfs:comment>
	</owl:Class>
	<owl:Class rdf:about="&android-1_6;OrgApacheHttpConnParams">
		<owl:equivalentClass rdf:resource="&android-1_5;OrgApacheHttpConnParams"/>
		<rdfs:subClassOf rdf:resource="&java;JavaAPIPart"/>
		<rdfs:seeAlso rdf:resource="&android-1_6;JavaLang"/>
		<rdfs:seeAlso rdf:resource="&android-1_6;OrgApacheHttp"/>
		<rdfs:seeAlso rdf:resource="&android-1_6;JavaUtil"/>
		<rdfs:seeAlso rdf:resource="&android-1_6;JavaNet"/>
		<rdfs:seeAlso rdf:resource="&android-1_6;OrgApacheHttpConnRouting"/>
		<rdfs:seeAlso rdf:resource="&android-1_6;OrgApacheHttpParams"/>
		<rdfs:comment xml:lang="en">Java API part implementing the org.apache.http.conn.params package for Android 1.6</rdfs:comment>
	</owl:Class>
	<owl:Class rdf:about="&android-1_6;OrgApacheHttpConnScheme">
		<owl:equivalentClass rdf:resource="&android-1_5;OrgApacheHttpConnScheme"/>
		<rdfs:subClassOf rdf:resource="&java;JavaAPIPart"/>
		<rdfs:seeAlso rdf:resource="&android-1_6;JavaLang"/>
		<rdfs:seeAlso rdf:resource="&android-1_6;OrgApacheHttp"/>
		<rdfs:seeAlso rdf:resource="&android-1_6;JavaUtil"/>
		<rdfs:seeAlso rdf:resource="&android-1_6;JavaNet"/>
		<rdfs:seeAlso rdf:resource="&android-1_6;OrgApacheHttpParams"/>
		<rdfs:comment xml:lang="en">Java API part implementing the org.apache.http.conn.scheme package for Android 1.6</rdfs:comment>
	</owl:Class>
	<owl:Class rdf:about="&android-1_6;OrgApacheHttpConnRouting">
		<owl:equivalentClass rdf:resource="&android-1_5;OrgApacheHttpConnRouting"/>
		<rdfs:subClassOf rdf:resource="&java;JavaAPIPart"/>
		<rdfs:seeAlso rdf:resource="&android-1_6;JavaLang"/>
		<rdfs:seeAlso rdf:resource="&android-1_6;OrgApacheHttp"/>
		<rdfs:seeAlso rdf:resource="&android-1_6;OrgApacheHttpProtocol"/>
		<rdfs:seeAlso rdf:resource="&android-1_6;JavaNet"/>
		<rdfs:comment xml:lang="en">Java API part implementing the org.apache.http.conn.routing package for Android 1.6</rdfs:comment>
	</owl:Class>
	<owl:Class rdf:about="&android-1_6;OrgApacheHttpConnSsl">
		<owl:equivalentClass rdf:resource="&android-1_5;OrgApacheHttpConnSsl"/>
		<rdfs:subClassOf rdf:resource="&java;JavaAPIPart"/>
		<rdfs:seeAlso rdf:resource="&android-1_6;JavaLang"/>
		<rdfs:seeAlso rdf:resource="&android-1_6;JavaSecurity"/>
		<rdfs:seeAlso rdf:resource="&android-1_6;JavaxNetSsl"/>
		<rdfs:seeAlso rdf:resource="&android-1_6;JavaNet"/>
		<rdfs:seeAlso rdf:resource="&android-1_6;JavaSecurityCert"/>
		<rdfs:seeAlso rdf:resource="&android-1_6;OrgApacheHttpConnScheme"/>
		<rdfs:seeAlso rdf:resource="&android-1_6;OrgApacheHttpParams"/>
		<rdfs:comment xml:lang="en">Java API part implementing the org.apache.http.conn.ssl package for Android 1.6</rdfs:comment>
	</owl:Class>
	<owl:Class rdf:about="&android-1_6;OrgApacheHttpConnUtil">
		<owl:equivalentClass rdf:resource="&android-1_5;OrgApacheHttpConnUtil"/>
		<rdfs:subClassOf rdf:resource="&java;JavaAPIPart"/>
		<rdfs:seeAlso rdf:resource="&android-1_6;JavaLang"/>
		<rdfs:comment xml:lang="en">Java API part implementing the org.apache.http.conn.util package for Android 1.6</rdfs:comment>
	</owl:Class>
	<owl:Class rdf:about="&android-1_6;OrgApacheHttpEntity">
		<owl:equivalentClass rdf:resource="&android-1_5;OrgApacheHttpEntity"/>
		<rdfs:subClassOf rdf:resource="&java;JavaAPIPart"/>
		<rdfs:seeAlso rdf:resource="&android-1_6;JavaLang"/>
		<rdfs:seeAlso rdf:resource="&android-1_6;OrgApacheHttp"/>
		<rdfs:seeAlso rdf:resource="&android-1_6;JavaIo"/>
		<rdfs:comment xml:lang="en">Java API part implementing the org.apache.http.entity package for Android 1.6</rdfs:comment>
	</owl:Class>
	<owl:Class rdf:about="&android-1_6;OrgApacheHttpMessage">
		<owl:equivalentClass rdf:resource="&android-1_5;OrgApacheHttpMessage"/>
		<rdfs:subClassOf rdf:resource="&java;JavaAPIPart"/>
		<rdfs:seeAlso rdf:resource="&android-1_6;JavaLang"/>
		<rdfs:seeAlso rdf:resource="&android-1_6;OrgApacheHttp"/>
		<rdfs:seeAlso rdf:resource="&android-1_6;OrgApacheHttpUtil"/>
		<rdfs:seeAlso rdf:resource="&android-1_6;OrgApacheHttpParams"/>
		<rdfs:seeAlso rdf:resource="&android-1_6;JavaUtil"/>
		<rdfs:comment xml:lang="en">Java API part implementing the org.apache.http.message package for Android 1.6</rdfs:comment>
	</owl:Class>
	<owl:Class rdf:about="&android-1_6;OrgApacheHttpImpl">
		<owl:equivalentClass rdf:resource="&android-1_5;OrgApacheHttpImpl"/>
		<rdfs:subClassOf rdf:resource="&java;JavaAPIPart"/>
		<rdfs:seeAlso rdf:resource="&android-1_6;OrgApacheHttpImplEntity"/>
		<rdfs:seeAlso rdf:resource="&android-1_6;OrgApacheHttp"/>
		<rdfs:seeAlso rdf:resource="&android-1_6;OrgApacheHttpProtocol"/>
		<rdfs:seeAlso rdf:resource="&android-1_6;JavaNet"/>
		<rdfs:seeAlso rdf:resource="&android-1_6;OrgApacheHttpParams"/>
		<rdfs:seeAlso rdf:resource="&android-1_6;JavaUtil"/>
		<rdfs:seeAlso rdf:resource="&android-1_6;OrgApacheHttpIo"/>
		<rdfs:seeAlso rdf:resource="&android-1_6;JavaLang"/>
		<rdfs:comment xml:lang="en">Java API part implementing the org.apache.http.impl package for Android 1.6</rdfs:comment>
	</owl:Class>
	<owl:Class rdf:about="&android-1_6;OrgApacheHttpImplEntity">
		<owl:equivalentClass rdf:resource="&android-1_5;OrgApacheHttpImplEntity"/>
		<rdfs:subClassOf rdf:resource="&java;JavaAPIPart"/>
		<rdfs:seeAlso rdf:resource="&android-1_6;JavaLang"/>
		<rdfs:seeAlso rdf:resource="&android-1_6;OrgApacheHttpEntity"/>
		<rdfs:seeAlso rdf:resource="&android-1_6;OrgApacheHttp"/>
		<rdfs:seeAlso rdf:resource="&android-1_6;JavaIo"/>
		<rdfs:seeAlso rdf:resource="&android-1_6;OrgApacheHttpIo"/>
		<rdfs:comment xml:lang="en">Java API part implementing the org.apache.http.impl.entity package for Android 1.6</rdfs:comment>
	</owl:Class>
	<owl:Class rdf:about="&android-1_6;OrgApacheHttpImplAuth">
		<owl:equivalentClass rdf:resource="&android-1_5;OrgApacheHttpImplAuth"/>
		<rdfs:subClassOf rdf:resource="&java;JavaAPIPart"/>
		<rdfs:seeAlso rdf:resource="&android-1_6;JavaLang"/>
		<rdfs:seeAlso rdf:resource="&android-1_6;OrgApacheHttp"/>
		<rdfs:seeAlso rdf:resource="&android-1_6;OrgApacheHttpUtil"/>
		<rdfs:seeAlso rdf:resource="&android-1_6;OrgApacheHttpParams"/>
		<rdfs:seeAlso rdf:resource="&android-1_6;OrgApacheHttpAuth"/>
		<rdfs:seeAlso rdf:resource="&android-1_6;JavaUtil"/>
		<rdfs:comment xml:lang="en">Java API part implementing the org.apache.http.impl.auth package for Android 1.6</rdfs:comment>
	</owl:Class>
	<owl:Class rdf:about="&android-1_6;OrgApacheHttpImplClient">
		<owl:equivalentClass rdf:resource="&android-1_5;OrgApacheHttpImplClient"/>
		<rdfs:subClassOf rdf:resource="&java;JavaAPIPart"/>
		<rdfs:seeAlso rdf:resource="&android-1_6;OrgApacheHttp"/>
		<rdfs:seeAlso rdf:resource="&android-1_6;OrgApacheHttpProtocol"/>
		<rdfs:seeAlso rdf:resource="&android-1_6;JavaNet"/>
		<rdfs:seeAlso rdf:resource="&android-1_6;OrgApacheHttpParams"/>
		<rdfs:seeAlso rdf:resource="&android-1_6;OrgApacheHttpAuth"/>
		<rdfs:seeAlso rdf:resource="&android-1_6;OrgApacheHttpCookie"/>
		<rdfs:seeAlso rdf:resource="&android-1_6;OrgApacheHttpMessage"/>
		<rdfs:seeAlso rdf:resource="&android-1_6;JavaUtil"/>
		<rdfs:seeAlso rdf:resource="&android-1_6;OrgApacheHttpClient"/>
		<rdfs:seeAlso rdf:resource="&android-1_6;JavaIo"/>
		<rdfs:seeAlso rdf:resource="&android-1_6;OrgApacheHttpClientMethods"/>
		<rdfs:seeAlso rdf:resource="&android-1_6;JavaLang"/>
		<rdfs:seeAlso rdf:resource="&android-1_6;OrgApacheHttpConnRouting"/>
		<rdfs:seeAlso rdf:resource="&android-1_6;OrgApacheHttpConn"/>
		<rdfs:comment xml:lang="en">Java API part implementing the org.apache.http.impl.client package for Android 1.6</rdfs:comment>
	</owl:Class>
	<owl:Class rdf:about="&android-1_6;OrgApacheHttpImplConn">
		<owl:equivalentClass rdf:resource="&android-1_5;OrgApacheHttpImplConn"/>
		<rdfs:subClassOf rdf:resource="&java;JavaAPIPart"/>
		<rdfs:seeAlso rdf:resource="&android-1_6;OrgApacheHttp"/>
		<rdfs:seeAlso rdf:resource="&android-1_6;OrgApacheHttpProtocol"/>
		<rdfs:seeAlso rdf:resource="&android-1_6;JavaxNetSsl"/>
		<rdfs:seeAlso rdf:resource="&android-1_6;JavaNet"/>
		<rdfs:seeAlso rdf:resource="&android-1_6;OrgApacheHttpParams"/>
		<rdfs:seeAlso rdf:resource="&android-1_6;OrgApacheHttpImpl"/>
		<rdfs:seeAlso rdf:resource="&android-1_6;OrgApacheHttpMessage"/>
		<rdfs:seeAlso rdf:resource="&android-1_6;JavaUtil"/>
		<rdfs:seeAlso rdf:resource="&android-1_6;JavaIo"/>
		<rdfs:seeAlso rdf:resource="&android-1_6;OrgApacheHttpIo"/>
		<rdfs:seeAlso rdf:resource="&android-1_6;OrgApacheCommonsLogging"/>
		<rdfs:seeAlso rdf:resource="&android-1_6;OrgApacheHttpImplIo"/>
		<rdfs:seeAlso rdf:resource="&android-1_6;JavaLang"/>
		<rdfs:seeAlso rdf:resource="&android-1_6;OrgApacheHttpUtil"/>
		<rdfs:seeAlso rdf:resource="&android-1_6;OrgApacheHttpConnRouting"/>
		<rdfs:seeAlso rdf:resource="&android-1_6;OrgApacheHttpConnScheme"/>
		<rdfs:seeAlso rdf:resource="&android-1_6;JavaUtilConcurrent"/>
		<rdfs:seeAlso rdf:resource="&android-1_6;OrgApacheHttpConn"/>
		<rdfs:comment xml:lang="en">Java API part implementing the org.apache.http.impl.conn package for Android 1.6</rdfs:comment>
	</owl:Class>
	<owl:Class rdf:about="&android-1_6;OrgApacheHttpImplConnTsccm">
		<owl:equivalentClass rdf:resource="&android-1_5;OrgApacheHttpImplConnTsccm"/>
		<rdfs:subClassOf rdf:resource="&java;JavaAPIPart"/>
		<rdfs:seeAlso rdf:resource="&android-1_6;OrgApacheHttpImplConn"/>
		<rdfs:seeAlso rdf:resource="&android-1_6;OrgApacheHttpParams"/>
		<rdfs:seeAlso rdf:resource="&android-1_6;JavaLangRef"/>
		<rdfs:seeAlso rdf:resource="&android-1_6;JavaUtil"/>
		<rdfs:seeAlso rdf:resource="&android-1_6;JavaUtilConcurrentLocks"/>
		<rdfs:seeAlso rdf:resource="&android-1_6;JavaLang"/>
		<rdfs:seeAlso rdf:resource="&android-1_6;OrgApacheHttpConnRouting"/>
		<rdfs:seeAlso rdf:resource="&android-1_6;OrgApacheHttpConnScheme"/>
		<rdfs:seeAlso rdf:resource="&android-1_6;JavaUtilConcurrent"/>
		<rdfs:seeAlso rdf:resource="&android-1_6;OrgApacheHttpConn"/>
		<rdfs:comment xml:lang="en">Java API part implementing the org.apache.http.impl.conn.tsccm package for Android 1.6</rdfs:comment>
	</owl:Class>
	<owl:Class rdf:about="&android-1_6;OrgApacheHttpImplIo">
		<owl:equivalentClass rdf:resource="&android-1_5;OrgApacheHttpImplIo"/>
		<rdfs:subClassOf rdf:resource="&java;JavaAPIPart"/>
		<rdfs:seeAlso rdf:resource="&android-1_6;JavaLang"/>
		<rdfs:seeAlso rdf:resource="&android-1_6;OrgApacheHttp"/>
		<rdfs:seeAlso rdf:resource="&android-1_6;OrgApacheHttpUtil"/>
		<rdfs:seeAlso rdf:resource="&android-1_6;JavaNet"/>
		<rdfs:seeAlso rdf:resource="&android-1_6;OrgApacheHttpParams"/>
		<rdfs:seeAlso rdf:resource="&android-1_6;OrgApacheHttpMessage"/>
		<rdfs:seeAlso rdf:resource="&android-1_6;JavaIo"/>
		<rdfs:seeAlso rdf:resource="&android-1_6;OrgApacheHttpIo"/>
		<rdfs:comment xml:lang="en">Java API part implementing the org.apache.http.impl.io package for Android 1.6</rdfs:comment>
	</owl:Class>
	<owl:Class rdf:about="&android-1_6;OrgApacheHttpImplCookie">
		<owl:equivalentClass rdf:resource="&android-1_5;OrgApacheHttpImplCookie"/>
		<rdfs:subClassOf rdf:resource="&java;JavaAPIPart"/>
		<rdfs:seeAlso rdf:resource="&android-1_6;JavaLang"/>
		<rdfs:seeAlso rdf:resource="&android-1_6;OrgApacheHttp"/>
		<rdfs:seeAlso rdf:resource="&android-1_6;OrgApacheHttpUtil"/>
		<rdfs:seeAlso rdf:resource="&android-1_6;OrgApacheHttpParams"/>
		<rdfs:seeAlso rdf:resource="&android-1_6;OrgApacheHttpCookie"/>
		<rdfs:seeAlso rdf:resource="&android-1_6;OrgApacheHttpMessage"/>
		<rdfs:seeAlso rdf:resource="&android-1_6;JavaUtil"/>
		<rdfs:comment xml:lang="en">Java API part implementing the org.apache.http.impl.cookie package for Android 1.6</rdfs:comment>
	</owl:Class>
	<owl:Class rdf:about="&android-1_6;OrgApacheHttpIo">
		<owl:equivalentClass rdf:resource="&android-1_5;OrgApacheHttpIo"/>
		<rdfs:subClassOf rdf:resource="&java;JavaAPIPart"/>
		<rdfs:seeAlso rdf:resource="&android-1_6;JavaLang"/>
		<rdfs:seeAlso rdf:resource="&android-1_6;OrgApacheHttp"/>
		<rdfs:seeAlso rdf:resource="&android-1_6;OrgApacheHttpUtil"/>
		<rdfs:comment xml:lang="en">Java API part implementing the org.apache.http.io package for Android 1.6</rdfs:comment>
	</owl:Class>
	<owl:Class rdf:about="&android-1_6;OrgJson">
		<owl:equivalentClass rdf:resource="&android-1_5;OrgJson"/>
		<rdfs:subClassOf rdf:resource="&java;JavaAPIPart"/>
		<rdfs:seeAlso rdf:resource="&android-1_6;JavaLang"/>
		<rdfs:seeAlso rdf:resource="&android-1_6;JavaUtil"/>
		<rdfs:comment xml:lang="en">Java API part implementing the org.json package for Android 1.6</rdfs:comment>
	</owl:Class>
	<owl:Class rdf:about="&android-1_6;JavaxMicroeditionKhronosOpengles">
		<owl:equivalentClass rdf:resource="&android-1_5;JavaxMicroeditionKhronosOpengles"/>
		<rdfs:subClassOf rdf:resource="&java;JavaAPIPart"/>
		<rdfs:seeAlso rdf:resource="&android-1_6;JavaNio"/>
		<rdfs:seeAlso rdf:resource="&android-1_6;JavaLang"/>
		<rdfs:comment xml:lang="en">Java API part implementing the javax.microedition.khronos.opengles package for Android 1.6</rdfs:comment>
	</owl:Class>
	<owl:Class rdf:about="&android-1_6;JavaxMicroeditionKhronosEgl">
		<owl:equivalentClass rdf:resource="&android-1_5;JavaxMicroeditionKhronosEgl"/>
		<rdfs:subClassOf rdf:resource="&java;JavaAPIPart"/>
		<rdfs:seeAlso rdf:resource="&android-1_6;JavaLang"/>
		<rdfs:seeAlso rdf:resource="&android-1_6;JavaxMicroeditionKhronosOpengles"/>
		<rdfs:comment xml:lang="en">Java API part implementing the javax.microedition.khronos.egl package for Android 1.6</rdfs:comment>
	</owl:Class>
	<owl:Class rdf:about="&android-1_6;JavaxNet">
		<owl:equivalentClass rdf:resource="&j2se-5_0;JavaxNet"/>
		<owl:equivalentClass rdf:resource="&android-1_5;JavaxNet"/>
		<rdfs:subClassOf rdf:resource="&java;JavaAPIPart"/>
		<rdfs:seeAlso rdf:resource="&android-1_6;JavaLang"/>
		<rdfs:seeAlso rdf:resource="&android-1_6;JavaNet"/>
		<rdfs:comment xml:lang="en">Java API part implementing the javax.net package for Android 1.6</rdfs:comment>
	</owl:Class>
	<owl:Class rdf:about="&android-1_6;JavaxNetSsl">
		<owl:equivalentClass rdf:resource="&j2se-5_0;JavaxNetSsl"/>
		<owl:equivalentClass rdf:resource="&android-1_5;JavaxNetSsl"/>
		<rdfs:subClassOf rdf:resource="&java;JavaAPIPart"/>
		<rdfs:seeAlso rdf:resource="&android-1_6;JavaNio"/>
		<rdfs:seeAlso rdf:resource="&android-1_6;JavaSecurity"/>
		<rdfs:seeAlso rdf:resource="&android-1_6;JavaSecurityCert"/>
		<rdfs:seeAlso rdf:resource="&android-1_6;JavaNet"/>
		<rdfs:seeAlso rdf:resource="&android-1_6;JavaUtil"/>
		<rdfs:seeAlso rdf:resource="&android-1_6;JavaIo"/>
		<rdfs:seeAlso rdf:resource="&android-1_6;JavaLang"/>
		<rdfs:seeAlso rdf:resource="&android-1_6;JavaxNet"/>
		<rdfs:comment xml:lang="en">Java API part implementing the javax.net.ssl package for Android 1.6</rdfs:comment>
	</owl:Class>
	<owl:Class rdf:about="&android-1_6;JavaxSecurityAuth">
		<owl:equivalentClass rdf:resource="&android-1_5;JavaxSecurityAuth"/>
		<rdfs:subClassOf rdf:resource="&java;JavaAPIPart"/>
		<rdfs:seeAlso rdf:resource="&android-1_6;JavaLang"/>
		<rdfs:seeAlso rdf:resource="&android-1_6;JavaSecurity"/>
		<rdfs:seeAlso rdf:resource="&android-1_6;JavaUtil"/>
		<rdfs:seeAlso rdf:resource="&android-1_6;JavaIo"/>
		<rdfs:comment xml:lang="en">Java API part implementing the javax.security.auth package for Android 1.6</rdfs:comment>
	</owl:Class>
	<owl:Class rdf:about="&android-1_6;JavaxSecurityAuthCallback">
		<owl:equivalentClass rdf:resource="&android-1_5;JavaxSecurityAuthCallback"/>
		<rdfs:subClassOf rdf:resource="&java;JavaAPIPart"/>
		<rdfs:seeAlso rdf:resource="&android-1_6;JavaLang"/>
		<rdfs:seeAlso rdf:resource="&android-1_6;JavaIo"/>
		<rdfs:comment xml:lang="en">Java API part implementing the javax.security.auth.callback package for Android 1.6</rdfs:comment>
	</owl:Class>
	<owl:Class rdf:about="&android-1_6;JavaxSecurityAuthX500">
		<owl:equivalentClass rdf:resource="&android-1_5;JavaxSecurityAuthX500"/>
		<rdfs:subClassOf rdf:resource="&java;JavaAPIPart"/>
		<rdfs:seeAlso rdf:resource="&android-1_6;JavaLang"/>
		<rdfs:seeAlso rdf:resource="&android-1_6;JavaIo"/>
		<rdfs:seeAlso rdf:resource="&android-1_6;JavaSecurity"/>
		<rdfs:comment xml:lang="en">Java API part implementing the javax.security.auth.x500 package for Android 1.6</rdfs:comment>
	</owl:Class>
	<owl:Class rdf:about="&android-1_6;JavaxSecurityAuthLogin">
		<owl:equivalentClass rdf:resource="&android-1_5;JavaxSecurityAuthLogin"/>
		<rdfs:subClassOf rdf:resource="&java;JavaAPIPart"/>
		<rdfs:seeAlso rdf:resource="&android-1_6;JavaLang"/>
		<rdfs:seeAlso rdf:resource="&android-1_6;JavaSecurity"/>
		<rdfs:comment xml:lang="en">Java API part implementing the javax.security.auth.login package for Android 1.6</rdfs:comment>
	</owl:Class>
	<owl:Class rdf:about="&android-1_6;JavaxSecurityCert">
		<owl:equivalentClass rdf:resource="&j2se-5_0;JavaxSecurityCert"/>
		<owl:equivalentClass rdf:resource="&android-1_5;JavaxSecurityCert"/>
		<rdfs:subClassOf rdf:resource="&java;JavaAPIPart"/>
		<rdfs:seeAlso rdf:resource="&android-1_6;JavaLang"/>
		<rdfs:seeAlso rdf:resource="&android-1_6;JavaUtil"/>
		<rdfs:seeAlso rdf:resource="&android-1_6;JavaIo"/>
		<rdfs:seeAlso rdf:resource="&android-1_6;JavaSecurity"/>
		<rdfs:seeAlso rdf:resource="&android-1_6;JavaMath"/>
		<rdfs:comment xml:lang="en">Java API part implementing the javax.security.cert package for Android 1.6</rdfs:comment>
	</owl:Class>
	<owl:Class rdf:about="&android-1_6;JavaxCrypto">
		<owl:equivalentClass rdf:resource="&j2se-5_0;JavaxCrypto"/>
		<owl:equivalentClass rdf:resource="&android-1_5;JavaxCrypto"/>
		<rdfs:subClassOf rdf:resource="&java;JavaAPIPart"/>
		<rdfs:seeAlso rdf:resource="&android-1_6;JavaNio"/>
		<rdfs:seeAlso rdf:resource="&android-1_6;JavaLang"/>
		<rdfs:seeAlso rdf:resource="&android-1_6;JavaSecurity"/>
		<rdfs:seeAlso rdf:resource="&android-1_6;JavaSecurityCert"/>
		<rdfs:seeAlso rdf:resource="&android-1_6;JavaSecuritySpec"/>
		<rdfs:seeAlso rdf:resource="&android-1_6;JavaIo"/>
		<rdfs:comment xml:lang="en">Java API part implementing the javax.crypto package for Android 1.6</rdfs:comment>
	</owl:Class>
	<owl:Class rdf:about="&android-1_6;JavaxCryptoInterfaces">
		<owl:equivalentClass rdf:resource="&j2se-5_0;JavaxCryptoInterfaces"/>
		<owl:equivalentClass rdf:resource="&android-1_5;JavaxCryptoInterfaces"/>
		<rdfs:subClassOf rdf:resource="&java;JavaAPIPart"/>
		<rdfs:seeAlso rdf:resource="&android-1_6;JavaxCryptoSpec"/>
		<rdfs:seeAlso rdf:resource="&android-1_6;JavaxCrypto"/>
		<rdfs:seeAlso rdf:resource="&android-1_6;JavaSecurity"/>
		<rdfs:seeAlso rdf:resource="&android-1_6;JavaMath"/>
		<rdfs:comment xml:lang="en">Java API part implementing the javax.crypto.interfaces package for Android 1.6</rdfs:comment>
	</owl:Class>
	<owl:Class rdf:about="&android-1_6;JavaxCryptoSpec">
		<owl:equivalentClass rdf:resource="&j2se-5_0;JavaxCryptoSpec"/>
		<owl:equivalentClass rdf:resource="&android-1_5;JavaxCryptoSpec"/>
		<rdfs:subClassOf rdf:resource="&java;JavaAPIPart"/>
		<rdfs:seeAlso rdf:resource="&android-1_6;JavaSecuritySpec"/>
		<rdfs:seeAlso rdf:resource="&android-1_6;JavaxCrypto"/>
		<rdfs:seeAlso rdf:resource="&android-1_6;JavaLang"/>
		<rdfs:seeAlso rdf:resource="&android-1_6;JavaIo"/>
		<rdfs:seeAlso rdf:resource="&android-1_6;JavaMath"/>
		<rdfs:comment xml:lang="en">Java API part implementing the javax.crypto.spec package for Android 1.6</rdfs:comment>
	</owl:Class>
	<owl:Class rdf:about="&android-1_6;JavaxSql">
		<owl:equivalentClass rdf:resource="&android-1_5;JavaxSql"/>
		<rdfs:subClassOf rdf:resource="&java;JavaAPIPart"/>
		<rdfs:seeAlso rdf:resource="&android-1_6;JavaLang"/>
		<rdfs:seeAlso rdf:resource="&android-1_6;JavaSql"/>
		<rdfs:seeAlso rdf:resource="&android-1_6;JavaMath"/>
		<rdfs:seeAlso rdf:resource="&android-1_6;JavaUtil"/>
		<rdfs:seeAlso rdf:resource="&android-1_6;JavaIo"/>
		<rdfs:comment xml:lang="en">Java API part implementing the javax.sql package for Android 1.6</rdfs:comment>
	</owl:Class>
	<owl:Class rdf:about="&android-1_6;JavaxXml">
		<owl:equivalentClass rdf:resource="&android-1_5;JavaxXml"/>
		<rdfs:subClassOf rdf:resource="&j2se-5_0;JavaxXml"/>
		<rdfs:seeAlso rdf:resource="&android-1_6;JavaLang"/>
		<rdfs:comment xml:lang="en">Java API part implementing the javax.xml package for Android 1.6</rdfs:comment>
	</owl:Class>
	<owl:Class rdf:about="&android-1_6;JavaxXmlParsers">
		<owl:equivalentClass rdf:resource="&android-1_5;JavaxXmlParsers"/>
		<rdfs:subClassOf rdf:resource="&java;JavaAPIPart"/>
		<rdfs:seeAlso rdf:resource="&android-1_6;JavaLang"/>
		<rdfs:seeAlso rdf:resource="&android-1_6;OrgXmlSaxHelpers"/>
		<rdfs:seeAlso rdf:resource="&android-1_6;OrgW3cDom"/>
		<rdfs:seeAlso rdf:resource="&android-1_6;JavaIo"/>
		<rdfs:seeAlso rdf:resource="&android-1_6;OrgXmlSax"/>
		<rdfs:comment xml:lang="en">Java API part implementing the javax.xml.parsers package for Android 1.6</rdfs:comment>
	</owl:Class>
	<owl:Class rdf:about="&android-1_6;JunitFramework">
		<owl:equivalentClass rdf:resource="&android-1_5;JunitFramework"/>
		<rdfs:subClassOf rdf:resource="&java;JavaAPIPart"/>
		<rdfs:seeAlso rdf:resource="&android-1_6;JavaLang"/>
		<rdfs:seeAlso rdf:resource="&android-1_6;JavaUtil"/>
		<rdfs:seeAlso rdf:resource="&android-1_6;JavaLangReflect"/>
		<rdfs:comment xml:lang="en">Java API part implementing the junit.framework package for Android 1.6</rdfs:comment>
	</owl:Class>
	<owl:Class rdf:about="&android-1_6;JunitRunner">
		<owl:equivalentClass rdf:resource="&android-1_5;JunitRunner"/>
		<rdfs:subClassOf rdf:resource="&java;JavaAPIPart"/>
		<rdfs:seeAlso rdf:resource="&android-1_6;JunitFramework"/>
		<rdfs:seeAlso rdf:resource="&android-1_6;JavaLang"/>
		<rdfs:seeAlso rdf:resource="&android-1_6;JavaUtil"/>
		<rdfs:comment xml:lang="en">Java API part implementing the junit.runner package for Android 1.6</rdfs:comment>
	</owl:Class>
	<owl:Class rdf:about="&android-1_6;DalvikAnnotation">
		<owl:equivalentClass rdf:resource="&android-1_5;DalvikAnnotation"/>
		<rdfs:subClassOf rdf:resource="&java;JavaAPIPart"/>
		<rdfs:seeAlso rdf:resource="&android-1_6;JavaLang"/>
		<rdfs:seeAlso rdf:resource="&android-1_6;JavaLangAnnotation"/>
		<rdfs:comment xml:lang="en">Java API part implementing the dalvik.annotation package for Android 1.6</rdfs:comment>
	</owl:Class>
	<owl:Class rdf:about="&android-1_6;DalvikBytecode">
		<owl:equivalentClass rdf:resource="&android-1_5;DalvikBytecode"/>
		<rdfs:subClassOf rdf:resource="&java;JavaAPIPart"/>
		<rdfs:comment xml:lang="en">Java API part implementing the dalvik.bytecode package for Android 1.6</rdfs:comment>
	</owl:Class>
	<owl:Class rdf:about="&android-1_6;DalvikSystem">
		<owl:equivalentClass rdf:resource="&android-1_5;DalvikSystem"/>
		<rdfs:subClassOf rdf:resource="&java;JavaAPIPart"/>
		<rdfs:seeAlso rdf:resource="&android-1_6;JavaLang"/>
		<rdfs:seeAlso rdf:resource="&android-1_6;JavaUtil"/>
		<rdfs:seeAlso rdf:resource="&android-1_6;JavaIo"/>
		<rdfs:seeAlso rdf:resource="&android-1_6;JavaNet"/>
		<rdfs:comment xml:lang="en">Java API part implementing the dalvik.system package for Android 1.6</rdfs:comment>
	</owl:Class>
	<owl:Class rdf:about="&android-1_6;AndroidAPI">
		<rdfs:subClassOf rdf:resource="&java;JavaAPI"/>
		<rdfs:comment xml:lang="en">JavaLibrary implementing the android package for Android 1.6</rdfs:comment>
		<rdfs:comment xml:lang="OWLManchester">platform:comprisesInterfacePart some Android</rdfs:comment>
	</owl:Class>
	<owl:Class rdf:about="&android-1_6;AndroidAccessibilityserviceAPI">
		<rdfs:subClassOf rdf:resource="&java;JavaAPI"/>
		<rdfs:comment xml:lang="en">JavaLibrary implementing the android.accessibilityservice package for Android 1.6</rdfs:comment>
		<rdfs:comment xml:lang="OWLManchester">platform:comprisesInterfacePart some AndroidAccessibilityservice</rdfs:comment>
	</owl:Class>
	<owl:Class rdf:about="&android-1_6;AndroidAppAPI">
		<rdfs:subClassOf rdf:resource="&android-1_5;AndroidAppAPI"/>
		<rdfs:comment xml:lang="en">JavaLibrary implementing the android.app package for Android 1.6</rdfs:comment>
		<rdfs:comment xml:lang="OWLManchester">platform:comprisesInterfacePart some AndroidApp</rdfs:comment>
	</owl:Class>
	<owl:Class rdf:about="&android-1_6;AndroidViewAPI">
		<rdfs:subClassOf rdf:resource="&android-1_5;AndroidViewAPI"/>
		<rdfs:comment xml:lang="en">JavaLibrary implementing the android.view package for Android 1.6</rdfs:comment>
		<rdfs:comment xml:lang="OWLManchester">platform:comprisesInterfacePart some AndroidView</rdfs:comment>
	</owl:Class>
	<owl:Class rdf:about="&android-1_6;AndroidViewAccessibilityAPI">
		<rdfs:subClassOf rdf:resource="&java;JavaAPI"/>
		<rdfs:comment xml:lang="en">JavaLibrary implementing the android.view.accessibility package for Android 1.6</rdfs:comment>
		<rdfs:comment xml:lang="OWLManchester">platform:comprisesInterfacePart some AndroidViewAccessibility</rdfs:comment>
	</owl:Class>
	<owl:Class rdf:about="&android-1_6;AndroidViewInputmethodAPI">
		<owl:equivalentClass rdf:resource="&android-1_5;AndroidViewInputmethodAPI"/>
		<rdfs:subClassOf rdf:resource="&java;JavaAPI"/>
		<rdfs:comment xml:lang="en">JavaLibrary implementing the android.view.inputmethod package for Android 1.6</rdfs:comment>
		<rdfs:comment xml:lang="OWLManchester">platform:comprisesInterfacePart some AndroidViewInputmethod</rdfs:comment>
	</owl:Class>
	<owl:Class rdf:about="&android-1_6;AndroidViewAnimationAPI">
		<rdfs:subClassOf rdf:resource="&android-1_5;AndroidViewAnimationAPI"/>
		<rdfs:comment xml:lang="en">JavaLibrary implementing the android.view.animation package for Android 1.6</rdfs:comment>
		<rdfs:comment xml:lang="OWLManchester">platform:comprisesInterfacePart some AndroidViewAnimation</rdfs:comment>
	</owl:Class>
	<owl:Class rdf:about="&android-1_6;AndroidContentAPI">
		<rdfs:subClassOf rdf:resource="&android-1_5;AndroidContentAPI"/>
		<rdfs:comment xml:lang="en">JavaLibrary implementing the android.content package for Android 1.6</rdfs:comment>
		<rdfs:comment xml:lang="OWLManchester">platform:comprisesInterfacePart some AndroidContent</rdfs:comment>
	</owl:Class>
	<owl:Class rdf:about="&android-1_6;AndroidContentResAPI">
		<rdfs:subClassOf rdf:resource="&android-1_5;AndroidContentResAPI"/>
		<rdfs:comment xml:lang="en">JavaLibrary implementing the android.content.res package for Android 1.6</rdfs:comment>
		<rdfs:comment xml:lang="OWLManchester">platform:comprisesInterfacePart some AndroidContentRes</rdfs:comment>
	</owl:Class>
	<owl:Class rdf:about="&android-1_6;AndroidContentPmAPI">
		<rdfs:subClassOf rdf:resource="&java;JavaAPI"/>
		<rdfs:comment xml:lang="en">JavaLibrary implementing the android.content.pm package for Android 1.6</rdfs:comment>
		<rdfs:comment xml:lang="OWLManchester">platform:comprisesInterfacePart some AndroidContentPm</rdfs:comment>
	</owl:Class>
	<owl:Class rdf:about="&android-1_6;AndroidOsAPI">
		<rdfs:subClassOf rdf:resource="&android-1_5;AndroidOsAPI"/>
		<rdfs:comment xml:lang="en">JavaLibrary implementing the android.os package for Android 1.6</rdfs:comment>
		<rdfs:comment xml:lang="OWLManchester">platform:comprisesInterfacePart some AndroidOs</rdfs:comment>
	</owl:Class>
	<owl:Class rdf:about="&android-1_6;AndroidGraphicsAPI">
		<rdfs:subClassOf rdf:resource="&android-1_5;AndroidGraphicsAPI"/>
		<rdfs:comment xml:lang="en">JavaLibrary implementing the android.graphics package for Android 1.6</rdfs:comment>
		<rdfs:comment xml:lang="OWLManchester">platform:comprisesInterfacePart some AndroidGraphics</rdfs:comment>
	</owl:Class>
	<owl:Class rdf:about="&android-1_6;AndroidGraphicsDrawableAPI">
		<rdfs:subClassOf rdf:resource="&android-1_5;AndroidGraphicsDrawableAPI"/>
		<rdfs:comment xml:lang="en">JavaLibrary implementing the android.graphics.drawable package for Android 1.6</rdfs:comment>
		<rdfs:comment xml:lang="OWLManchester">platform:comprisesInterfacePart some AndroidGraphicsDrawable</rdfs:comment>
	</owl:Class>
	<owl:Class rdf:about="&android-1_6;AndroidGraphicsDrawableShapesAPI">
		<owl:equivalentClass rdf:resource="&android-1_5;AndroidGraphicsDrawableShapesAPI"/>
		<rdfs:subClassOf rdf:resource="&java;JavaAPI"/>
		<rdfs:comment xml:lang="en">JavaLibrary implementing the android.graphics.drawable.shapes package for Android 1.6</rdfs:comment>
		<rdfs:comment xml:lang="OWLManchester">platform:comprisesInterfacePart some AndroidGraphicsDrawableShapes</rdfs:comment>
	</owl:Class>
	<owl:Class rdf:about="&android-1_6;AndroidNetAPI">
		<owl:equivalentClass rdf:resource="&android-1_5;AndroidNetAPI"/>
		<rdfs:subClassOf rdf:resource="&java;JavaAPI"/>
		<rdfs:comment xml:lang="en">JavaLibrary implementing the android.net package for Android 1.6</rdfs:comment>
		<rdfs:comment xml:lang="OWLManchester">platform:comprisesInterfacePart some AndroidNet</rdfs:comment>
	</owl:Class>
	<owl:Class rdf:about="&android-1_6;AndroidNetHttpAPI">
		<owl:equivalentClass rdf:resource="&android-1_5;AndroidNetHttpAPI"/>
		<rdfs:subClassOf rdf:resource="&java;JavaAPI"/>
		<rdfs:comment xml:lang="en">JavaLibrary implementing the android.net.http package for Android 1.6</rdfs:comment>
		<rdfs:comment xml:lang="OWLManchester">platform:comprisesInterfacePart some AndroidNetHttp</rdfs:comment>
	</owl:Class>
	<owl:Class rdf:about="&android-1_6;AndroidNetWifiAPI">
		<rdfs:subClassOf rdf:resource="&android-1_5;AndroidNetWifiAPI"/>
		<rdfs:comment xml:lang="en">JavaLibrary implementing the android.net.wifi package for Android 1.6</rdfs:comment>
		<rdfs:comment xml:lang="OWLManchester">platform:comprisesInterfacePart some AndroidNetWifi</rdfs:comment>
	</owl:Class>
	<owl:Class rdf:about="&android-1_6;AndroidDatabaseAPI">
		<owl:equivalentClass rdf:resource="&android-1_5;AndroidDatabaseAPI"/>
		<rdfs:subClassOf rdf:resource="&java;JavaAPI"/>
		<rdfs:comment xml:lang="en">JavaLibrary implementing the android.database package for Android 1.6</rdfs:comment>
		<rdfs:comment xml:lang="OWLManchester">platform:comprisesInterfacePart some AndroidDatabase</rdfs:comment>
	</owl:Class>
	<owl:Class rdf:about="&android-1_6;AndroidDatabaseSqliteAPI">
		<owl:equivalentClass rdf:resource="&android-1_5;AndroidDatabaseSqliteAPI"/>
		<rdfs:subClassOf rdf:resource="&java;JavaAPI"/>
		<rdfs:comment xml:lang="en">JavaLibrary implementing the android.database.sqlite package for Android 1.6</rdfs:comment>
		<rdfs:comment xml:lang="OWLManchester">platform:comprisesInterfacePart some AndroidDatabaseSqlite</rdfs:comment>
	</owl:Class>
	<owl:Class rdf:about="&android-1_6;AndroidUtilAPI">
		<rdfs:subClassOf rdf:resource="&android-1_5;AndroidUtilAPI"/>
		<rdfs:comment xml:lang="en">JavaLibrary implementing the android.util package for Android 1.6</rdfs:comment>
		<rdfs:comment xml:lang="OWLManchester">platform:comprisesInterfacePart some AndroidUtil</rdfs:comment>
	</owl:Class>
	<owl:Class rdf:about="&android-1_6;AndroidWidgetAPI">
		<rdfs:subClassOf rdf:resource="&android-1_5;AndroidWidgetAPI"/>
		<rdfs:comment xml:lang="en">JavaLibrary implementing the android.widget package for Android 1.6</rdfs:comment>
		<rdfs:comment xml:lang="OWLManchester">platform:comprisesInterfacePart some AndroidWidget</rdfs:comment>
	</owl:Class>
	<owl:Class rdf:about="&android-1_6;AndroidAppwidgetAPI">
		<rdfs:subClassOf rdf:resource="&android-1_5;AndroidAppwidgetAPI"/>
		<rdfs:comment xml:lang="en">JavaLibrary implementing the android.appwidget package for Android 1.6</rdfs:comment>
		<rdfs:comment xml:lang="OWLManchester">platform:comprisesInterfacePart some AndroidAppwidget</rdfs:comment>
	</owl:Class>
	<owl:Class rdf:about="&android-1_6;AndroidGestureAPI">
		<rdfs:subClassOf rdf:resource="&java;JavaAPI"/>
		<rdfs:comment xml:lang="en">JavaLibrary implementing the android.gesture package for Android 1.6</rdfs:comment>
		<rdfs:comment xml:lang="OWLManchester">platform:comprisesInterfacePart some AndroidGesture</rdfs:comment>
	</owl:Class>
	<owl:Class rdf:about="&android-1_6;AndroidHardwareAPI">
		<owl:equivalentClass rdf:resource="&android-1_5;AndroidHardwareAPI"/>
		<rdfs:subClassOf rdf:resource="&java;JavaAPI"/>
		<rdfs:comment xml:lang="en">JavaLibrary implementing the android.hardware package for Android 1.6</rdfs:comment>
		<rdfs:comment xml:lang="OWLManchester">platform:comprisesInterfacePart some AndroidHardware</rdfs:comment>
	</owl:Class>
	<owl:Class rdf:about="&android-1_6;AndroidInputmethodserviceAPI">
		<rdfs:subClassOf rdf:resource="&android-1_5;AndroidInputmethodserviceAPI"/>
		<rdfs:comment xml:lang="en">JavaLibrary implementing the android.inputmethodservice package for Android 1.6</rdfs:comment>
		<rdfs:comment xml:lang="OWLManchester">platform:comprisesInterfacePart some AndroidInputmethodservice</rdfs:comment>
	</owl:Class>
	<owl:Class rdf:about="&android-1_6;AndroidLocationAPI">
		<rdfs:subClassOf rdf:resource="&android-1_5;AndroidLocationAPI"/>
		<rdfs:comment xml:lang="en">JavaLibrary implementing the android.location package for Android 1.6</rdfs:comment>
		<rdfs:comment xml:lang="OWLManchester">platform:comprisesInterfacePart some AndroidLocation</rdfs:comment>
	</owl:Class>
	<owl:Class rdf:about="&android-1_6;AndroidMediaAPI">
		<rdfs:subClassOf rdf:resource="&android-1_5;AndroidMediaAPI"/>
		<rdfs:comment xml:lang="en">JavaLibrary implementing the android.media package for Android 1.6</rdfs:comment>
		<rdfs:comment xml:lang="OWLManchester">platform:comprisesInterfacePart some AndroidMedia</rdfs:comment>
	</owl:Class>
	<owl:Class rdf:about="&android-1_6;AndroidOpenglAPI">
		<rdfs:subClassOf rdf:resource="&android-1_5;AndroidOpenglAPI"/>
		<rdfs:comment xml:lang="en">JavaLibrary implementing the android.opengl package for Android 1.6</rdfs:comment>
		<rdfs:comment xml:lang="OWLManchester">platform:comprisesInterfacePart some AndroidOpengl</rdfs:comment>
	</owl:Class>
	<owl:Class rdf:about="&android-1_6;AndroidPreferenceAPI">
		<rdfs:subClassOf rdf:resource="&android-1_5;AndroidPreferenceAPI"/>
		<rdfs:comment xml:lang="en">JavaLibrary implementing the android.preference package for Android 1.6</rdfs:comment>
		<rdfs:comment xml:lang="OWLManchester">platform:comprisesInterfacePart some AndroidPreference</rdfs:comment>
	</owl:Class>
	<owl:Class rdf:about="&android-1_6;AndroidProviderAPI">
		<rdfs:subClassOf rdf:resource="&android-1_5;AndroidProviderAPI"/>
		<rdfs:comment xml:lang="en">JavaLibrary implementing the android.provider package for Android 1.6</rdfs:comment>
		<rdfs:comment xml:lang="OWLManchester">platform:comprisesInterfacePart some AndroidProvider</rdfs:comment>
	</owl:Class>
	<owl:Class rdf:about="&android-1_6;AndroidWebkitAPI">
		<rdfs:subClassOf rdf:resource="&android-1_5;AndroidWebkitAPI"/>
		<rdfs:comment xml:lang="en">JavaLibrary implementing the android.webkit package for Android 1.6</rdfs:comment>
		<rdfs:comment xml:lang="OWLManchester">platform:comprisesInterfacePart some AndroidWebkit</rdfs:comment>
	</owl:Class>
	<owl:Class rdf:about="&android-1_6;AndroidSaxAPI">
		<owl:equivalentClass rdf:resource="&android-1_5;AndroidSaxAPI"/>
		<rdfs:subClassOf rdf:resource="&java;JavaAPI"/>
		<rdfs:comment xml:lang="en">JavaLibrary implementing the android.sax package for Android 1.6</rdfs:comment>
		<rdfs:comment xml:lang="OWLManchester">platform:comprisesInterfacePart some AndroidSax</rdfs:comment>
	</owl:Class>
	<owl:Class rdf:about="&android-1_6;AndroidSpeechAPI">
		<owl:equivalentClass rdf:resource="&android-1_5;AndroidSpeechAPI"/>
		<rdfs:subClassOf rdf:resource="&java;JavaAPI"/>
		<rdfs:comment xml:lang="en">JavaLibrary implementing the android.speech package for Android 1.6</rdfs:comment>
		<rdfs:comment xml:lang="OWLManchester">platform:comprisesInterfacePart some AndroidSpeech</rdfs:comment>
	</owl:Class>
	<owl:Class rdf:about="&android-1_6;AndroidSpeechTtsAPI">
		<rdfs:subClassOf rdf:resource="&java;JavaAPI"/>
		<rdfs:comment xml:lang="en">JavaLibrary implementing the android.speech.tts package for Android 1.6</rdfs:comment>
		<rdfs:comment xml:lang="OWLManchester">platform:comprisesInterfacePart some AndroidSpeechTts</rdfs:comment>
	</owl:Class>
	<owl:Class rdf:about="&android-1_6;AndroidTelephonyAPI">
		<rdfs:subClassOf rdf:resource="&android-1_5;AndroidTelephonyAPI"/>
		<rdfs:comment xml:lang="en">JavaLibrary implementing the android.telephony package for Android 1.6</rdfs:comment>
		<rdfs:comment xml:lang="OWLManchester">platform:comprisesInterfacePart some AndroidTelephony</rdfs:comment>
	</owl:Class>
	<owl:Class rdf:about="&android-1_6;AndroidTelephonyGsmAPI">
		<rdfs:subClassOf rdf:resource="&java;JavaAPI"/>
		<rdfs:comment xml:lang="en">JavaLibrary implementing the android.telephony.gsm package for Android 1.6</rdfs:comment>
		<rdfs:comment xml:lang="OWLManchester">platform:comprisesInterfacePart some AndroidTelephonyGsm</rdfs:comment>
	</owl:Class>
	<owl:Class rdf:about="&android-1_6;AndroidTextAPI">
		<owl:equivalentClass rdf:resource="&android-1_5;AndroidTextAPI"/>
		<rdfs:subClassOf rdf:resource="&java;JavaAPI"/>
		<rdfs:comment xml:lang="en">JavaLibrary implementing the android.text package for Android 1.6</rdfs:comment>
		<rdfs:comment xml:lang="OWLManchester">platform:comprisesInterfacePart some AndroidText</rdfs:comment>
	</owl:Class>
	<owl:Class rdf:about="&android-1_6;AndroidTextFormatAPI">
		<owl:equivalentClass rdf:resource="&android-1_5;AndroidTextFormatAPI"/>
		<rdfs:subClassOf rdf:resource="&java;JavaAPI"/>
		<rdfs:comment xml:lang="en">JavaLibrary implementing the android.text.format package for Android 1.6</rdfs:comment>
		<rdfs:comment xml:lang="OWLManchester">platform:comprisesInterfacePart some AndroidTextFormat</rdfs:comment>
	</owl:Class>
	<owl:Class rdf:about="&android-1_6;AndroidTextMethodAPI">
		<rdfs:subClassOf rdf:resource="&android-1_5;AndroidTextMethodAPI"/>
		<rdfs:comment xml:lang="en">JavaLibrary implementing the android.text.method package for Android 1.6</rdfs:comment>
		<rdfs:comment xml:lang="OWLManchester">platform:comprisesInterfacePart some AndroidTextMethod</rdfs:comment>
	</owl:Class>
	<owl:Class rdf:about="&android-1_6;AndroidTextStyleAPI">
		<rdfs:subClassOf rdf:resource="&android-1_5;AndroidTextStyleAPI"/>
		<rdfs:comment xml:lang="en">JavaLibrary implementing the android.text.style package for Android 1.6</rdfs:comment>
		<rdfs:comment xml:lang="OWLManchester">platform:comprisesInterfacePart some AndroidTextStyle</rdfs:comment>
	</owl:Class>
	<owl:Class rdf:about="&android-1_6;AndroidTextUtilAPI">
		<owl:equivalentClass rdf:resource="&android-1_5;AndroidTextUtilAPI"/>
		<rdfs:subClassOf rdf:resource="&java;JavaAPI"/>
		<rdfs:comment xml:lang="en">JavaLibrary implementing the android.text.util package for Android 1.6</rdfs:comment>
		<rdfs:comment xml:lang="OWLManchester">platform:comprisesInterfacePart some AndroidTextUtil</rdfs:comment>
	</owl:Class>
	<owl:Class rdf:about="&android-1_6;AndroidTestAPI">
		<rdfs:subClassOf rdf:resource="&android-1_5;AndroidTestAPI"/>
		<rdfs:comment xml:lang="en">JavaLibrary implementing the android.test package for Android 1.6</rdfs:comment>
		<rdfs:comment xml:lang="OWLManchester">platform:comprisesInterfacePart some AndroidTest</rdfs:comment>
	</owl:Class>
	<owl:Class rdf:about="&android-1_6;AndroidTestMockAPI">
		<rdfs:subClassOf rdf:resource="&java;JavaAPI"/>
		<rdfs:comment xml:lang="en">JavaLibrary implementing the android.test.mock package for Android 1.6</rdfs:comment>
		<rdfs:comment xml:lang="OWLManchester">platform:comprisesInterfacePart some AndroidTestMock</rdfs:comment>
	</owl:Class>
	<owl:Class rdf:about="&android-1_6;AndroidTestSuitebuilderAPI">
		<owl:equivalentClass rdf:resource="&android-1_5;AndroidTestSuitebuilderAPI"/>
		<rdfs:subClassOf rdf:resource="&java;JavaAPI"/>
		<rdfs:comment xml:lang="en">JavaLibrary implementing the android.test.suitebuilder package for Android 1.6</rdfs:comment>
		<rdfs:comment xml:lang="OWLManchester">platform:comprisesInterfacePart some AndroidTestSuitebuilder</rdfs:comment>
	</owl:Class>
	<owl:Class rdf:about="&android-1_6;AndroidTestSuitebuilderAnnotationAPI">
		<owl:equivalentClass rdf:resource="&android-1_5;AndroidTestSuitebuilderAnnotationAPI"/>
		<rdfs:subClassOf rdf:resource="&java;JavaAPI"/>
		<rdfs:comment xml:lang="en">JavaLibrary implementing the android.test.suitebuilder.annotation package for Android 1.6</rdfs:comment>
		<rdfs:comment xml:lang="OWLManchester">platform:comprisesInterfacePart some AndroidTestSuitebuilderAnnotation</rdfs:comment>
	</owl:Class>
	<owl:Class rdf:about="&android-1_6;JavaLangAPI">
		<owl:equivalentClass rdf:resource="&android-1_5;JavaLangAPI"/>
		<rdfs:subClassOf rdf:resource="&j2se-5_0;JavaLangAPI"/>
		<rdfs:comment xml:lang="en">JavaLibrary implementing the java.lang package for Android 1.6</rdfs:comment>
		<rdfs:comment xml:lang="OWLManchester">platform:comprisesInterfacePart some JavaLang</rdfs:comment>
	</owl:Class>
	<owl:Class rdf:about="&android-1_6;JavaLangAnnotationAPI">
		<owl:equivalentClass rdf:resource="&j2se-5_0;JavaLangAnnotationAPI"/>
		<owl:equivalentClass rdf:resource="&android-1_5;JavaLangAnnotationAPI"/>
		<rdfs:subClassOf rdf:resource="&java;JavaAPI"/>
		<rdfs:comment xml:lang="en">JavaLibrary implementing the java.lang.annotation package for Android 1.6</rdfs:comment>
		<rdfs:comment xml:lang="OWLManchester">platform:comprisesInterfacePart some JavaLangAnnotation</rdfs:comment>
	</owl:Class>
	<owl:Class rdf:about="&android-1_6;JavaLangReflectAPI">
		<owl:equivalentClass rdf:resource="&j2se-5_0;JavaLangReflectAPI"/>
		<owl:equivalentClass rdf:resource="&android-1_5;JavaLangReflectAPI"/>
		<rdfs:subClassOf rdf:resource="&java;JavaAPI"/>
		<rdfs:comment xml:lang="en">JavaLibrary implementing the java.lang.reflect package for Android 1.6</rdfs:comment>
		<rdfs:comment xml:lang="OWLManchester">platform:comprisesInterfacePart some JavaLangReflect</rdfs:comment>
	</owl:Class>
	<owl:Class rdf:about="&android-1_6;JavaLangRefAPI">
		<owl:equivalentClass rdf:resource="&j2se-5_0;JavaLangRefAPI"/>
		<owl:equivalentClass rdf:resource="&android-1_5;JavaLangRefAPI"/>
		<rdfs:subClassOf rdf:resource="&java;JavaAPI"/>
		<rdfs:comment xml:lang="en">JavaLibrary implementing the java.lang.ref package for Android 1.6</rdfs:comment>
		<rdfs:comment xml:lang="OWLManchester">platform:comprisesInterfacePart some JavaLangRef</rdfs:comment>
	</owl:Class>
	<owl:Class rdf:about="&android-1_6;JavaUtilAPI">
		<owl:equivalentClass rdf:resource="&j2se-5_0;JavaUtilAPI"/>
		<owl:equivalentClass rdf:resource="&android-1_5;JavaUtilAPI"/>
		<rdfs:subClassOf rdf:resource="&java;JavaAPI"/>
		<rdfs:comment xml:lang="en">JavaLibrary implementing the java.util package for Android 1.6</rdfs:comment>
		<rdfs:comment xml:lang="OWLManchester">platform:comprisesInterfacePart some JavaUtil</rdfs:comment>
	</owl:Class>
	<owl:Class rdf:about="&android-1_6;JavaUtilConcurrentAPI">
		<owl:equivalentClass rdf:resource="&j2se-5_0;JavaUtilConcurrentAPI"/>
		<owl:equivalentClass rdf:resource="&android-1_5;JavaUtilConcurrentAPI"/>
		<rdfs:subClassOf rdf:resource="&java;JavaAPI"/>
		<rdfs:comment xml:lang="en">JavaLibrary implementing the java.util.concurrent package for Android 1.6</rdfs:comment>
		<rdfs:comment xml:lang="OWLManchester">platform:comprisesInterfacePart some JavaUtilConcurrent</rdfs:comment>
	</owl:Class>
	<owl:Class rdf:about="&android-1_6;JavaUtilConcurrentAtomicAPI">
		<owl:equivalentClass rdf:resource="&j2se-5_0;JavaUtilConcurrentAtomicAPI"/>
		<owl:equivalentClass rdf:resource="&android-1_5;JavaUtilConcurrentAtomicAPI"/>
		<rdfs:subClassOf rdf:resource="&java;JavaAPI"/>
		<rdfs:comment xml:lang="en">JavaLibrary implementing the java.util.concurrent.atomic package for Android 1.6</rdfs:comment>
		<rdfs:comment xml:lang="OWLManchester">platform:comprisesInterfacePart some JavaUtilConcurrentAtomic</rdfs:comment>
	</owl:Class>
	<owl:Class rdf:about="&android-1_6;JavaUtilConcurrentLocksAPI">
		<owl:equivalentClass rdf:resource="&j2se-5_0;JavaUtilConcurrentLocksAPI"/>
		<owl:equivalentClass rdf:resource="&android-1_5;JavaUtilConcurrentLocksAPI"/>
		<rdfs:subClassOf rdf:resource="&java;JavaAPI"/>
		<rdfs:comment xml:lang="en">JavaLibrary implementing the java.util.concurrent.locks package for Android 1.6</rdfs:comment>
		<rdfs:comment xml:lang="OWLManchester">platform:comprisesInterfacePart some JavaUtilConcurrentLocks</rdfs:comment>
	</owl:Class>
	<owl:Class rdf:about="&android-1_6;JavaUtilRegexAPI">
		<owl:equivalentClass rdf:resource="&j2se-5_0;JavaUtilRegexAPI"/>
		<owl:equivalentClass rdf:resource="&android-1_5;JavaUtilRegexAPI"/>
		<rdfs:subClassOf rdf:resource="&java;JavaAPI"/>
		<rdfs:comment xml:lang="en">JavaLibrary implementing the java.util.regex package for Android 1.6</rdfs:comment>
		<rdfs:comment xml:lang="OWLManchester">platform:comprisesInterfacePart some JavaUtilRegex</rdfs:comment>
	</owl:Class>
	<owl:Class rdf:about="&android-1_6;JavaUtilJarAPI">
		<owl:equivalentClass rdf:resource="&j2se-5_0;JavaUtilJarAPI"/>
		<owl:equivalentClass rdf:resource="&android-1_5;JavaUtilJarAPI"/>
		<rdfs:subClassOf rdf:resource="&java;JavaAPI"/>
		<rdfs:comment xml:lang="en">JavaLibrary implementing the java.util.jar package for Android 1.6</rdfs:comment>
		<rdfs:comment xml:lang="OWLManchester">platform:comprisesInterfacePart some JavaUtilJar</rdfs:comment>
	</owl:Class>
	<owl:Class rdf:about="&android-1_6;JavaUtilZipAPI">
		<owl:equivalentClass rdf:resource="&j2se-5_0;JavaUtilZipAPI"/>
		<owl:equivalentClass rdf:resource="&android-1_5;JavaUtilZipAPI"/>
		<rdfs:subClassOf rdf:resource="&java;JavaAPI"/>
		<rdfs:comment xml:lang="en">JavaLibrary implementing the java.util.zip package for Android 1.6</rdfs:comment>
		<rdfs:comment xml:lang="OWLManchester">platform:comprisesInterfacePart some JavaUtilZip</rdfs:comment>
	</owl:Class>
	<owl:Class rdf:about="&android-1_6;JavaUtilLoggingAPI">
		<owl:equivalentClass rdf:resource="&j2se-5_0;JavaUtilLoggingAPI"/>
		<owl:equivalentClass rdf:resource="&android-1_5;JavaUtilLoggingAPI"/>
		<rdfs:subClassOf rdf:resource="&java;JavaAPI"/>
		<rdfs:comment xml:lang="en">JavaLibrary implementing the java.util.logging package for Android 1.6</rdfs:comment>
		<rdfs:comment xml:lang="OWLManchester">platform:comprisesInterfacePart some JavaUtilLogging</rdfs:comment>
	</owl:Class>
	<owl:Class rdf:about="&android-1_6;JavaUtilPrefsAPI">
		<owl:equivalentClass rdf:resource="&j2se-5_0;JavaUtilPrefsAPI"/>
		<owl:equivalentClass rdf:resource="&android-1_5;JavaUtilPrefsAPI"/>
		<rdfs:subClassOf rdf:resource="&java;JavaAPI"/>
		<rdfs:comment xml:lang="en">JavaLibrary implementing the java.util.prefs package for Android 1.6</rdfs:comment>
		<rdfs:comment xml:lang="OWLManchester">platform:comprisesInterfacePart some JavaUtilPrefs</rdfs:comment>
	</owl:Class>
	<owl:Class rdf:about="&android-1_6;JavaIoAPI">
		<owl:equivalentClass rdf:resource="&j2se-5_0;JavaIoAPI"/>
		<owl:equivalentClass rdf:resource="&android-1_5;JavaIoAPI"/>
		<rdfs:subClassOf rdf:resource="&java;JavaAPI"/>
		<rdfs:comment xml:lang="en">JavaLibrary implementing the java.io package for Android 1.6</rdfs:comment>
		<rdfs:comment xml:lang="OWLManchester">platform:comprisesInterfacePart some JavaIo</rdfs:comment>
	</owl:Class>
	<owl:Class rdf:about="&android-1_6;JavaNioAPI">
		<owl:equivalentClass rdf:resource="&j2se-5_0;JavaNioAPI"/>
		<owl:equivalentClass rdf:resource="&android-1_5;JavaNioAPI"/>
		<rdfs:subClassOf rdf:resource="&java;JavaAPI"/>
		<rdfs:comment xml:lang="en">JavaLibrary implementing the java.nio package for Android 1.6</rdfs:comment>
		<rdfs:comment xml:lang="OWLManchester">platform:comprisesInterfacePart some JavaNio</rdfs:comment>
	</owl:Class>
	<owl:Class rdf:about="&android-1_6;JavaNioChannelsAPI">
		<owl:equivalentClass rdf:resource="&j2se-5_0;JavaNioChannelsAPI"/>
		<owl:equivalentClass rdf:resource="&android-1_5;JavaNioChannelsAPI"/>
		<rdfs:subClassOf rdf:resource="&java;JavaAPI"/>
		<rdfs:comment xml:lang="en">JavaLibrary implementing the java.nio.channels package for Android 1.6</rdfs:comment>
		<rdfs:comment xml:lang="OWLManchester">platform:comprisesInterfacePart some JavaNioChannels</rdfs:comment>
	</owl:Class>
	<owl:Class rdf:about="&android-1_6;JavaNioChannelsSpiAPI">
		<owl:equivalentClass rdf:resource="&j2se-5_0;JavaNioChannelsSpiAPI"/>
		<owl:equivalentClass rdf:resource="&android-1_5;JavaNioChannelsSpiAPI"/>
		<rdfs:subClassOf rdf:resource="&java;JavaAPI"/>
		<rdfs:comment xml:lang="en">JavaLibrary implementing the java.nio.channels.spi package for Android 1.6</rdfs:comment>
		<rdfs:comment xml:lang="OWLManchester">platform:comprisesInterfacePart some JavaNioChannelsSpi</rdfs:comment>
	</owl:Class>
	<owl:Class rdf:about="&android-1_6;JavaNioCharsetAPI">
		<owl:equivalentClass rdf:resource="&j2se-5_0;JavaNioCharsetAPI"/>
		<owl:equivalentClass rdf:resource="&android-1_5;JavaNioCharsetAPI"/>
		<rdfs:subClassOf rdf:resource="&java;JavaAPI"/>
		<rdfs:comment xml:lang="en">JavaLibrary implementing the java.nio.charset package for Android 1.6</rdfs:comment>
		<rdfs:comment xml:lang="OWLManchester">platform:comprisesInterfacePart some JavaNioCharset</rdfs:comment>
	</owl:Class>
	<owl:Class rdf:about="&android-1_6;JavaNioCharsetSpiAPI">
		<owl:equivalentClass rdf:resource="&j2se-5_0;JavaNioCharsetSpiAPI"/>
		<owl:equivalentClass rdf:resource="&android-1_5;JavaNioCharsetSpiAPI"/>
		<rdfs:subClassOf rdf:resource="&java;JavaAPI"/>
		<rdfs:comment xml:lang="en">JavaLibrary implementing the java.nio.charset.spi package for Android 1.6</rdfs:comment>
		<rdfs:comment xml:lang="OWLManchester">platform:comprisesInterfacePart some JavaNioCharsetSpi</rdfs:comment>
	</owl:Class>
	<owl:Class rdf:about="&android-1_6;JavaNetAPI">
		<owl:equivalentClass rdf:resource="&j2se-5_0;JavaNetAPI"/>
		<owl:equivalentClass rdf:resource="&android-1_5;JavaNetAPI"/>
		<rdfs:subClassOf rdf:resource="&java;JavaAPI"/>
		<rdfs:comment xml:lang="en">JavaLibrary implementing the java.net package for Android 1.6</rdfs:comment>
		<rdfs:comment xml:lang="OWLManchester">platform:comprisesInterfacePart some JavaNet</rdfs:comment>
	</owl:Class>
	<owl:Class rdf:about="&android-1_6;JavaSecurityAPI">
		<owl:equivalentClass rdf:resource="&j2se-5_0;JavaSecurityAPI"/>
		<owl:equivalentClass rdf:resource="&android-1_5;JavaSecurityAPI"/>
		<rdfs:subClassOf rdf:resource="&java;JavaAPI"/>
		<rdfs:comment xml:lang="en">JavaLibrary implementing the java.security package for Android 1.6</rdfs:comment>
		<rdfs:comment xml:lang="OWLManchester">platform:comprisesInterfacePart some JavaSecurity</rdfs:comment>
	</owl:Class>
	<owl:Class rdf:about="&android-1_6;JavaSecurityCertAPI">
		<owl:equivalentClass rdf:resource="&j2se-5_0;JavaSecurityCertAPI"/>
		<owl:equivalentClass rdf:resource="&android-1_5;JavaSecurityCertAPI"/>
		<rdfs:subClassOf rdf:resource="&java;JavaAPI"/>
		<rdfs:comment xml:lang="en">JavaLibrary implementing the java.security.cert package for Android 1.6</rdfs:comment>
		<rdfs:comment xml:lang="OWLManchester">platform:comprisesInterfacePart some JavaSecurityCert</rdfs:comment>
	</owl:Class>
	<owl:Class rdf:about="&android-1_6;JavaSecuritySpecAPI">
		<owl:equivalentClass rdf:resource="&j2se-5_0;JavaSecuritySpecAPI"/>
		<owl:equivalentClass rdf:resource="&android-1_5;JavaSecuritySpecAPI"/>
		<rdfs:subClassOf rdf:resource="&java;JavaAPI"/>
		<rdfs:comment xml:lang="en">JavaLibrary implementing the java.security.spec package for Android 1.6</rdfs:comment>
		<rdfs:comment xml:lang="OWLManchester">platform:comprisesInterfacePart some JavaSecuritySpec</rdfs:comment>
	</owl:Class>
	<owl:Class rdf:about="&android-1_6;JavaSecurityAclAPI">
		<owl:equivalentClass rdf:resource="&j2se-5_0;JavaSecurityAclAPI"/>
		<owl:equivalentClass rdf:resource="&android-1_5;JavaSecurityAclAPI"/>
		<rdfs:subClassOf rdf:resource="&java;JavaAPI"/>
		<rdfs:comment xml:lang="en">JavaLibrary implementing the java.security.acl package for Android 1.6</rdfs:comment>
		<rdfs:comment xml:lang="OWLManchester">platform:comprisesInterfacePart some JavaSecurityAcl</rdfs:comment>
	</owl:Class>
	<owl:Class rdf:about="&android-1_6;JavaSecurityInterfacesAPI">
		<owl:equivalentClass rdf:resource="&j2se-5_0;JavaSecurityInterfacesAPI"/>
		<owl:equivalentClass rdf:resource="&android-1_5;JavaSecurityInterfacesAPI"/>
		<rdfs:subClassOf rdf:resource="&java;JavaAPI"/>
		<rdfs:comment xml:lang="en">JavaLibrary implementing the java.security.interfaces package for Android 1.6</rdfs:comment>
		<rdfs:comment xml:lang="OWLManchester">platform:comprisesInterfacePart some JavaSecurityInterfaces</rdfs:comment>
	</owl:Class>
	<owl:Class rdf:about="&android-1_6;JavaTextAPI">
		<owl:equivalentClass rdf:resource="&j2se-5_0;JavaTextAPI"/>
		<owl:equivalentClass rdf:resource="&android-1_5;JavaTextAPI"/>
		<rdfs:subClassOf rdf:resource="&java;JavaAPI"/>
		<rdfs:comment xml:lang="en">JavaLibrary implementing the java.text package for Android 1.6</rdfs:comment>
		<rdfs:comment xml:lang="OWLManchester">platform:comprisesInterfacePart some JavaText</rdfs:comment>
	</owl:Class>
	<owl:Class rdf:about="&android-1_6;JavaAwtFontAPI">
		<owl:equivalentClass rdf:resource="&android-1_5;JavaAwtFontAPI"/>
		<rdfs:subClassOf rdf:resource="&java;JavaAPI"/>
		<rdfs:comment xml:lang="en">JavaLibrary implementing the java.awt.font package for Android 1.6</rdfs:comment>
		<rdfs:comment xml:lang="OWLManchester">platform:comprisesInterfacePart some JavaAwtFont</rdfs:comment>
	</owl:Class>
	<owl:Class rdf:about="&android-1_6;JavaBeansAPI">
		<owl:equivalentClass rdf:resource="&android-1_5;JavaBeansAPI"/>
		<rdfs:subClassOf rdf:resource="&java;JavaAPI"/>
		<rdfs:comment xml:lang="en">JavaLibrary implementing the java.beans package for Android 1.6</rdfs:comment>
		<rdfs:comment xml:lang="OWLManchester">platform:comprisesInterfacePart some JavaBeans</rdfs:comment>
	</owl:Class>
	<owl:Class rdf:about="&android-1_6;JavaMathAPI">
		<owl:equivalentClass rdf:resource="&j2se-5_0;JavaMathAPI"/>
		<owl:equivalentClass rdf:resource="&android-1_5;JavaMathAPI"/>
		<rdfs:subClassOf rdf:resource="&java;JavaAPI"/>
		<rdfs:comment xml:lang="en">JavaLibrary implementing the java.math package for Android 1.6</rdfs:comment>
		<rdfs:comment xml:lang="OWLManchester">platform:comprisesInterfacePart some JavaMath</rdfs:comment>
	</owl:Class>
	<owl:Class rdf:about="&android-1_6;JavaSqlAPI">
		<owl:equivalentClass rdf:resource="&j2se-5_0;JavaSqlAPI"/>
		<owl:equivalentClass rdf:resource="&android-1_5;JavaSqlAPI"/>
		<rdfs:subClassOf rdf:resource="&java;JavaAPI"/>
		<rdfs:comment xml:lang="en">JavaLibrary implementing the java.sql package for Android 1.6</rdfs:comment>
		<rdfs:comment xml:lang="OWLManchester">platform:comprisesInterfacePart some JavaSql</rdfs:comment>
	</owl:Class>
	<owl:Class rdf:about="&android-1_6;OrgXmlpullV1API">
		<owl:equivalentClass rdf:resource="&android-1_5;OrgXmlpullV1API"/>
		<rdfs:subClassOf rdf:resource="&java;JavaAPI"/>
		<rdfs:comment xml:lang="en">JavaLibrary implementing the org.xmlpull.v1 package for Android 1.6</rdfs:comment>
		<rdfs:comment xml:lang="OWLManchester">platform:comprisesInterfacePart some OrgXmlpullV1</rdfs:comment>
	</owl:Class>
	<owl:Class rdf:about="&android-1_6;OrgXmlpullV1Sax2API">
		<owl:equivalentClass rdf:resource="&android-1_5;OrgXmlpullV1Sax2API"/>
		<rdfs:subClassOf rdf:resource="&java;JavaAPI"/>
		<rdfs:comment xml:lang="en">JavaLibrary implementing the org.xmlpull.v1.sax2 package for Android 1.6</rdfs:comment>
		<rdfs:comment xml:lang="OWLManchester">platform:comprisesInterfacePart some OrgXmlpullV1Sax2</rdfs:comment>
	</owl:Class>
	<owl:Class rdf:about="&android-1_6;OrgXmlSaxAPI">
		<owl:equivalentClass rdf:resource="&j2se-5_0;OrgXmlSaxAPI"/>
		<owl:equivalentClass rdf:resource="&android-1_5;OrgXmlSaxAPI"/>
		<rdfs:subClassOf rdf:resource="&java;JavaAPI"/>
		<rdfs:comment xml:lang="en">JavaLibrary implementing the org.xml.sax package for Android 1.6</rdfs:comment>
		<rdfs:comment xml:lang="OWLManchester">platform:comprisesInterfacePart some OrgXmlSax</rdfs:comment>
	</owl:Class>
	<owl:Class rdf:about="&android-1_6;OrgXmlSaxHelpersAPI">
		<owl:equivalentClass rdf:resource="&j2se-5_0;OrgXmlSaxHelpersAPI"/>
		<owl:equivalentClass rdf:resource="&android-1_5;OrgXmlSaxHelpersAPI"/>
		<rdfs:subClassOf rdf:resource="&java;JavaAPI"/>
		<rdfs:comment xml:lang="en">JavaLibrary implementing the org.xml.sax.helpers package for Android 1.6</rdfs:comment>
		<rdfs:comment xml:lang="OWLManchester">platform:comprisesInterfacePart some OrgXmlSaxHelpers</rdfs:comment>
	</owl:Class>
	<owl:Class rdf:about="&android-1_6;OrgXmlSaxExtAPI">
		<owl:equivalentClass rdf:resource="&j2se-5_0;OrgXmlSaxExtAPI"/>
		<owl:equivalentClass rdf:resource="&android-1_5;OrgXmlSaxExtAPI"/>
		<rdfs:subClassOf rdf:resource="&java;JavaAPI"/>
		<rdfs:comment xml:lang="en">JavaLibrary implementing the org.xml.sax.ext package for Android 1.6</rdfs:comment>
		<rdfs:comment xml:lang="OWLManchester">platform:comprisesInterfacePart some OrgXmlSaxExt</rdfs:comment>
	</owl:Class>
	<owl:Class rdf:about="&android-1_6;OrgW3cDomAPI">
		<owl:equivalentClass rdf:resource="&android-1_5;OrgW3cDomAPI"/>
		<rdfs:subClassOf rdf:resource="&java;JavaAPI"/>
		<rdfs:comment xml:lang="en">JavaLibrary implementing the org.w3c.dom package for Android 1.6</rdfs:comment>
		<rdfs:comment xml:lang="OWLManchester">platform:comprisesInterfacePart some OrgW3cDom</rdfs:comment>
	</owl:Class>
	<owl:Class rdf:about="&android-1_6;OrgApacheCommonsLoggingAPI">
		<owl:equivalentClass rdf:resource="&android-1_5;OrgApacheCommonsLoggingAPI"/>
		<rdfs:subClassOf rdf:resource="&java;JavaAPI"/>
		<rdfs:comment xml:lang="en">JavaLibrary implementing the org.apache.commons.logging package for Android 1.6</rdfs:comment>
		<rdfs:comment xml:lang="OWLManchester">platform:comprisesInterfacePart some OrgApacheCommonsLogging</rdfs:comment>
	</owl:Class>
	<owl:Class rdf:about="&android-1_6;OrgApacheHttpAPI">
		<owl:equivalentClass rdf:resource="&android-1_5;OrgApacheHttpAPI"/>
		<rdfs:subClassOf rdf:resource="&java;JavaAPI"/>
		<rdfs:comment xml:lang="en">JavaLibrary implementing the org.apache.http package for Android 1.6</rdfs:comment>
		<rdfs:comment xml:lang="OWLManchester">platform:comprisesInterfacePart some OrgApacheHttp</rdfs:comment>
	</owl:Class>
	<owl:Class rdf:about="&android-1_6;OrgApacheHttpProtocolAPI">
		<owl:equivalentClass rdf:resource="&android-1_5;OrgApacheHttpProtocolAPI"/>
		<rdfs:subClassOf rdf:resource="&java;JavaAPI"/>
		<rdfs:comment xml:lang="en">JavaLibrary implementing the org.apache.http.protocol package for Android 1.6</rdfs:comment>
		<rdfs:comment xml:lang="OWLManchester">platform:comprisesInterfacePart some OrgApacheHttpProtocol</rdfs:comment>
	</owl:Class>
	<owl:Class rdf:about="&android-1_6;OrgApacheHttpUtilAPI">
		<owl:equivalentClass rdf:resource="&android-1_5;OrgApacheHttpUtilAPI"/>
		<rdfs:subClassOf rdf:resource="&java;JavaAPI"/>
		<rdfs:comment xml:lang="en">JavaLibrary implementing the org.apache.http.util package for Android 1.6</rdfs:comment>
		<rdfs:comment xml:lang="OWLManchester">platform:comprisesInterfacePart some OrgApacheHttpUtil</rdfs:comment>
	</owl:Class>
	<owl:Class rdf:about="&android-1_6;OrgApacheHttpParamsAPI">
		<owl:equivalentClass rdf:resource="&android-1_5;OrgApacheHttpParamsAPI"/>
		<rdfs:subClassOf rdf:resource="&java;JavaAPI"/>
		<rdfs:comment xml:lang="en">JavaLibrary implementing the org.apache.http.params package for Android 1.6</rdfs:comment>
		<rdfs:comment xml:lang="OWLManchester">platform:comprisesInterfacePart some OrgApacheHttpParams</rdfs:comment>
	</owl:Class>
	<owl:Class rdf:about="&android-1_6;OrgApacheHttpAuthAPI">
		<owl:equivalentClass rdf:resource="&android-1_5;OrgApacheHttpAuthAPI"/>
		<rdfs:subClassOf rdf:resource="&java;JavaAPI"/>
		<rdfs:comment xml:lang="en">JavaLibrary implementing the org.apache.http.auth package for Android 1.6</rdfs:comment>
		<rdfs:comment xml:lang="OWLManchester">platform:comprisesInterfacePart some OrgApacheHttpAuth</rdfs:comment>
	</owl:Class>
	<owl:Class rdf:about="&android-1_6;OrgApacheHttpAuthParamsAPI">
		<owl:equivalentClass rdf:resource="&android-1_5;OrgApacheHttpAuthParamsAPI"/>
		<rdfs:subClassOf rdf:resource="&java;JavaAPI"/>
		<rdfs:comment xml:lang="en">JavaLibrary implementing the org.apache.http.auth.params package for Android 1.6</rdfs:comment>
		<rdfs:comment xml:lang="OWLManchester">platform:comprisesInterfacePart some OrgApacheHttpAuthParams</rdfs:comment>
	</owl:Class>
	<owl:Class rdf:about="&android-1_6;OrgApacheHttpClientAPI">
		<owl:equivalentClass rdf:resource="&android-1_5;OrgApacheHttpClientAPI"/>
		<rdfs:subClassOf rdf:resource="&java;JavaAPI"/>
		<rdfs:comment xml:lang="en">JavaLibrary implementing the org.apache.http.client package for Android 1.6</rdfs:comment>
		<rdfs:comment xml:lang="OWLManchester">platform:comprisesInterfacePart some OrgApacheHttpClient</rdfs:comment>
	</owl:Class>
	<owl:Class rdf:about="&android-1_6;OrgApacheHttpClientMethodsAPI">
		<owl:equivalentClass rdf:resource="&android-1_5;OrgApacheHttpClientMethodsAPI"/>
		<rdfs:subClassOf rdf:resource="&java;JavaAPI"/>
		<rdfs:comment xml:lang="en">JavaLibrary implementing the org.apache.http.client.methods package for Android 1.6</rdfs:comment>
		<rdfs:comment xml:lang="OWLManchester">platform:comprisesInterfacePart some OrgApacheHttpClientMethods</rdfs:comment>
	</owl:Class>
	<owl:Class rdf:about="&android-1_6;OrgApacheHttpClientEntityAPI">
		<owl:equivalentClass rdf:resource="&android-1_5;OrgApacheHttpClientEntityAPI"/>
		<rdfs:subClassOf rdf:resource="&java;JavaAPI"/>
		<rdfs:comment xml:lang="en">JavaLibrary implementing the org.apache.http.client.entity package for Android 1.6</rdfs:comment>
		<rdfs:comment xml:lang="OWLManchester">platform:comprisesInterfacePart some OrgApacheHttpClientEntity</rdfs:comment>
	</owl:Class>
	<owl:Class rdf:about="&android-1_6;OrgApacheHttpClientParamsAPI">
		<owl:equivalentClass rdf:resource="&android-1_5;OrgApacheHttpClientParamsAPI"/>
		<rdfs:subClassOf rdf:resource="&java;JavaAPI"/>
		<rdfs:comment xml:lang="en">JavaLibrary implementing the org.apache.http.client.params package for Android 1.6</rdfs:comment>
		<rdfs:comment xml:lang="OWLManchester">platform:comprisesInterfacePart some OrgApacheHttpClientParams</rdfs:comment>
	</owl:Class>
	<owl:Class rdf:about="&android-1_6;OrgApacheHttpClientProtocolAPI">
		<owl:equivalentClass rdf:resource="&android-1_5;OrgApacheHttpClientProtocolAPI"/>
		<rdfs:subClassOf rdf:resource="&java;JavaAPI"/>
		<rdfs:comment xml:lang="en">JavaLibrary implementing the org.apache.http.client.protocol package for Android 1.6</rdfs:comment>
		<rdfs:comment xml:lang="OWLManchester">platform:comprisesInterfacePart some OrgApacheHttpClientProtocol</rdfs:comment>
	</owl:Class>
	<owl:Class rdf:about="&android-1_6;OrgApacheHttpClientUtilsAPI">
		<owl:equivalentClass rdf:resource="&android-1_5;OrgApacheHttpClientUtilsAPI"/>
		<rdfs:subClassOf rdf:resource="&java;JavaAPI"/>
		<rdfs:comment xml:lang="en">JavaLibrary implementing the org.apache.http.client.utils package for Android 1.6</rdfs:comment>
		<rdfs:comment xml:lang="OWLManchester">platform:comprisesInterfacePart some OrgApacheHttpClientUtils</rdfs:comment>
	</owl:Class>
	<owl:Class rdf:about="&android-1_6;OrgApacheHttpCookieAPI">
		<owl:equivalentClass rdf:resource="&android-1_5;OrgApacheHttpCookieAPI"/>
		<rdfs:subClassOf rdf:resource="&java;JavaAPI"/>
		<rdfs:comment xml:lang="en">JavaLibrary implementing the org.apache.http.cookie package for Android 1.6</rdfs:comment>
		<rdfs:comment xml:lang="OWLManchester">platform:comprisesInterfacePart some OrgApacheHttpCookie</rdfs:comment>
	</owl:Class>
	<owl:Class rdf:about="&android-1_6;OrgApacheHttpCookieParamsAPI">
		<owl:equivalentClass rdf:resource="&android-1_5;OrgApacheHttpCookieParamsAPI"/>
		<rdfs:subClassOf rdf:resource="&java;JavaAPI"/>
		<rdfs:comment xml:lang="en">JavaLibrary implementing the org.apache.http.cookie.params package for Android 1.6</rdfs:comment>
		<rdfs:comment xml:lang="OWLManchester">platform:comprisesInterfacePart some OrgApacheHttpCookieParams</rdfs:comment>
	</owl:Class>
	<owl:Class rdf:about="&android-1_6;OrgApacheHttpConnAPI">
		<owl:equivalentClass rdf:resource="&android-1_5;OrgApacheHttpConnAPI"/>
		<rdfs:subClassOf rdf:resource="&java;JavaAPI"/>
		<rdfs:comment xml:lang="en">JavaLibrary implementing the org.apache.http.conn package for Android 1.6</rdfs:comment>
		<rdfs:comment xml:lang="OWLManchester">platform:comprisesInterfacePart some OrgApacheHttpConn</rdfs:comment>
	</owl:Class>
	<owl:Class rdf:about="&android-1_6;OrgApacheHttpConnParamsAPI">
		<owl:equivalentClass rdf:resource="&android-1_5;OrgApacheHttpConnParamsAPI"/>
		<rdfs:subClassOf rdf:resource="&java;JavaAPI"/>
		<rdfs:comment xml:lang="en">JavaLibrary implementing the org.apache.http.conn.params package for Android 1.6</rdfs:comment>
		<rdfs:comment xml:lang="OWLManchester">platform:comprisesInterfacePart some OrgApacheHttpConnParams</rdfs:comment>
	</owl:Class>
	<owl:Class rdf:about="&android-1_6;OrgApacheHttpConnSchemeAPI">
		<owl:equivalentClass rdf:resource="&android-1_5;OrgApacheHttpConnSchemeAPI"/>
		<rdfs:subClassOf rdf:resource="&java;JavaAPI"/>
		<rdfs:comment xml:lang="en">JavaLibrary implementing the org.apache.http.conn.scheme package for Android 1.6</rdfs:comment>
		<rdfs:comment xml:lang="OWLManchester">platform:comprisesInterfacePart some OrgApacheHttpConnScheme</rdfs:comment>
	</owl:Class>
	<owl:Class rdf:about="&android-1_6;OrgApacheHttpConnRoutingAPI">
		<owl:equivalentClass rdf:resource="&android-1_5;OrgApacheHttpConnRoutingAPI"/>
		<rdfs:subClassOf rdf:resource="&java;JavaAPI"/>
		<rdfs:comment xml:lang="en">JavaLibrary implementing the org.apache.http.conn.routing package for Android 1.6</rdfs:comment>
		<rdfs:comment xml:lang="OWLManchester">platform:comprisesInterfacePart some OrgApacheHttpConnRouting</rdfs:comment>
	</owl:Class>
	<owl:Class rdf:about="&android-1_6;OrgApacheHttpConnSslAPI">
		<owl:equivalentClass rdf:resource="&android-1_5;OrgApacheHttpConnSslAPI"/>
		<rdfs:subClassOf rdf:resource="&java;JavaAPI"/>
		<rdfs:comment xml:lang="en">JavaLibrary implementing the org.apache.http.conn.ssl package for Android 1.6</rdfs:comment>
		<rdfs:comment xml:lang="OWLManchester">platform:comprisesInterfacePart some OrgApacheHttpConnSsl</rdfs:comment>
	</owl:Class>
	<owl:Class rdf:about="&android-1_6;OrgApacheHttpConnUtilAPI">
		<owl:equivalentClass rdf:resource="&android-1_5;OrgApacheHttpConnUtilAPI"/>
		<rdfs:subClassOf rdf:resource="&java;JavaAPI"/>
		<rdfs:comment xml:lang="en">JavaLibrary implementing the org.apache.http.conn.util package for Android 1.6</rdfs:comment>
		<rdfs:comment xml:lang="OWLManchester">platform:comprisesInterfacePart some OrgApacheHttpConnUtil</rdfs:comment>
	</owl:Class>
	<owl:Class rdf:about="&android-1_6;OrgApacheHttpEntityAPI">
		<owl:equivalentClass rdf:resource="&android-1_5;OrgApacheHttpEntityAPI"/>
		<rdfs:subClassOf rdf:resource="&java;JavaAPI"/>
		<rdfs:comment xml:lang="en">JavaLibrary implementing the org.apache.http.entity package for Android 1.6</rdfs:comment>
		<rdfs:comment xml:lang="OWLManchester">platform:comprisesInterfacePart some OrgApacheHttpEntity</rdfs:comment>
	</owl:Class>
	<owl:Class rdf:about="&android-1_6;OrgApacheHttpMessageAPI">
		<owl:equivalentClass rdf:resource="&android-1_5;OrgApacheHttpMessageAPI"/>
		<rdfs:subClassOf rdf:resource="&java;JavaAPI"/>
		<rdfs:comment xml:lang="en">JavaLibrary implementing the org.apache.http.message package for Android 1.6</rdfs:comment>
		<rdfs:comment xml:lang="OWLManchester">platform:comprisesInterfacePart some OrgApacheHttpMessage</rdfs:comment>
	</owl:Class>
	<owl:Class rdf:about="&android-1_6;OrgApacheHttpImplAPI">
		<owl:equivalentClass rdf:resource="&android-1_5;OrgApacheHttpImplAPI"/>
		<rdfs:subClassOf rdf:resource="&java;JavaAPI"/>
		<rdfs:comment xml:lang="en">JavaLibrary implementing the org.apache.http.impl package for Android 1.6</rdfs:comment>
		<rdfs:comment xml:lang="OWLManchester">platform:comprisesInterfacePart some OrgApacheHttpImpl</rdfs:comment>
	</owl:Class>
	<owl:Class rdf:about="&android-1_6;OrgApacheHttpImplEntityAPI">
		<owl:equivalentClass rdf:resource="&android-1_5;OrgApacheHttpImplEntityAPI"/>
		<rdfs:subClassOf rdf:resource="&java;JavaAPI"/>
		<rdfs:comment xml:lang="en">JavaLibrary implementing the org.apache.http.impl.entity package for Android 1.6</rdfs:comment>
		<rdfs:comment xml:lang="OWLManchester">platform:comprisesInterfacePart some OrgApacheHttpImplEntity</rdfs:comment>
	</owl:Class>
	<owl:Class rdf:about="&android-1_6;OrgApacheHttpImplAuthAPI">
		<owl:equivalentClass rdf:resource="&android-1_5;OrgApacheHttpImplAuthAPI"/>
		<rdfs:subClassOf rdf:resource="&java;JavaAPI"/>
		<rdfs:comment xml:lang="en">JavaLibrary implementing the org.apache.http.impl.auth package for Android 1.6</rdfs:comment>
		<rdfs:comment xml:lang="OWLManchester">platform:comprisesInterfacePart some OrgApacheHttpImplAuth</rdfs:comment>
	</owl:Class>
	<owl:Class rdf:about="&android-1_6;OrgApacheHttpImplClientAPI">
		<owl:equivalentClass rdf:resource="&android-1_5;OrgApacheHttpImplClientAPI"/>
		<rdfs:subClassOf rdf:resource="&java;JavaAPI"/>
		<rdfs:comment xml:lang="en">JavaLibrary implementing the org.apache.http.impl.client package for Android 1.6</rdfs:comment>
		<rdfs:comment xml:lang="OWLManchester">platform:comprisesInterfacePart some OrgApacheHttpImplClient</rdfs:comment>
	</owl:Class>
	<owl:Class rdf:about="&android-1_6;OrgApacheHttpImplConnAPI">
		<owl:equivalentClass rdf:resource="&android-1_5;OrgApacheHttpImplConnAPI"/>
		<rdfs:subClassOf rdf:resource="&java;JavaAPI"/>
		<rdfs:comment xml:lang="en">JavaLibrary implementing the org.apache.http.impl.conn package for Android 1.6</rdfs:comment>
		<rdfs:comment xml:lang="OWLManchester">platform:comprisesInterfacePart some OrgApacheHttpImplConn</rdfs:comment>
	</owl:Class>
	<owl:Class rdf:about="&android-1_6;OrgApacheHttpImplConnTsccmAPI">
		<owl:equivalentClass rdf:resource="&android-1_5;OrgApacheHttpImplConnTsccmAPI"/>
		<rdfs:subClassOf rdf:resource="&java;JavaAPI"/>
		<rdfs:comment xml:lang="en">JavaLibrary implementing the org.apache.http.impl.conn.tsccm package for Android 1.6</rdfs:comment>
		<rdfs:comment xml:lang="OWLManchester">platform:comprisesInterfacePart some OrgApacheHttpImplConnTsccm</rdfs:comment>
	</owl:Class>
	<owl:Class rdf:about="&android-1_6;OrgApacheHttpImplIoAPI">
		<owl:equivalentClass rdf:resource="&android-1_5;OrgApacheHttpImplIoAPI"/>
		<rdfs:subClassOf rdf:resource="&java;JavaAPI"/>
		<rdfs:comment xml:lang="en">JavaLibrary implementing the org.apache.http.impl.io package for Android 1.6</rdfs:comment>
		<rdfs:comment xml:lang="OWLManchester">platform:comprisesInterfacePart some OrgApacheHttpImplIo</rdfs:comment>
	</owl:Class>
	<owl:Class rdf:about="&android-1_6;OrgApacheHttpImplCookieAPI">
		<owl:equivalentClass rdf:resource="&android-1_5;OrgApacheHttpImplCookieAPI"/>
		<rdfs:subClassOf rdf:resource="&java;JavaAPI"/>
		<rdfs:comment xml:lang="en">JavaLibrary implementing the org.apache.http.impl.cookie package for Android 1.6</rdfs:comment>
		<rdfs:comment xml:lang="OWLManchester">platform:comprisesInterfacePart some OrgApacheHttpImplCookie</rdfs:comment>
	</owl:Class>
	<owl:Class rdf:about="&android-1_6;OrgApacheHttpIoAPI">
		<owl:equivalentClass rdf:resource="&android-1_5;OrgApacheHttpIoAPI"/>
		<rdfs:subClassOf rdf:resource="&java;JavaAPI"/>
		<rdfs:comment xml:lang="en">JavaLibrary implementing the org.apache.http.io package for Android 1.6</rdfs:comment>
		<rdfs:comment xml:lang="OWLManchester">platform:comprisesInterfacePart some OrgApacheHttpIo</rdfs:comment>
	</owl:Class>
	<owl:Class rdf:about="&android-1_6;OrgJsonAPI">
		<owl:equivalentClass rdf:resource="&android-1_5;OrgJsonAPI"/>
		<rdfs:subClassOf rdf:resource="&java;JavaAPI"/>
		<rdfs:comment xml:lang="en">JavaLibrary implementing the org.json package for Android 1.6</rdfs:comment>
		<rdfs:comment xml:lang="OWLManchester">platform:comprisesInterfacePart some OrgJson</rdfs:comment>
	</owl:Class>
	<owl:Class rdf:about="&android-1_6;JavaxMicroeditionKhronosOpenglesAPI">
		<owl:equivalentClass rdf:resource="&android-1_5;JavaxMicroeditionKhronosOpenglesAPI"/>
		<rdfs:subClassOf rdf:resource="&java;JavaAPI"/>
		<rdfs:comment xml:lang="en">JavaLibrary implementing the javax.microedition.khronos.opengles package for Android 1.6</rdfs:comment>
		<rdfs:comment xml:lang="OWLManchester">platform:comprisesInterfacePart some JavaxMicroeditionKhronosOpengles</rdfs:comment>
	</owl:Class>
	<owl:Class rdf:about="&android-1_6;JavaxMicroeditionKhronosEglAPI">
		<owl:equivalentClass rdf:resource="&android-1_5;JavaxMicroeditionKhronosEglAPI"/>
		<rdfs:subClassOf rdf:resource="&java;JavaAPI"/>
		<rdfs:comment xml:lang="en">JavaLibrary implementing the javax.microedition.khronos.egl package for Android 1.6</rdfs:comment>
		<rdfs:comment xml:lang="OWLManchester">platform:comprisesInterfacePart some JavaxMicroeditionKhronosEgl</rdfs:comment>
	</owl:Class>
	<owl:Class rdf:about="&android-1_6;JavaxNetAPI">
		<owl:equivalentClass rdf:resource="&j2se-5_0;JavaxNetAPI"/>
		<owl:equivalentClass rdf:resource="&android-1_5;JavaxNetAPI"/>
		<rdfs:subClassOf rdf:resource="&java;JavaAPI"/>
		<rdfs:comment xml:lang="en">JavaLibrary implementing the javax.net package for Android 1.6</rdfs:comment>
		<rdfs:comment xml:lang="OWLManchester">platform:comprisesInterfacePart some JavaxNet</rdfs:comment>
	</owl:Class>
	<owl:Class rdf:about="&android-1_6;JavaxNetSslAPI">
		<owl:equivalentClass rdf:resource="&j2se-5_0;JavaxNetSslAPI"/>
		<owl:equivalentClass rdf:resource="&android-1_5;JavaxNetSslAPI"/>
		<rdfs:subClassOf rdf:resource="&java;JavaAPI"/>
		<rdfs:comment xml:lang="en">JavaLibrary implementing the javax.net.ssl package for Android 1.6</rdfs:comment>
		<rdfs:comment xml:lang="OWLManchester">platform:comprisesInterfacePart some JavaxNetSsl</rdfs:comment>
	</owl:Class>
	<owl:Class rdf:about="&android-1_6;JavaxSecurityAuthAPI">
		<owl:equivalentClass rdf:resource="&android-1_5;JavaxSecurityAuthAPI"/>
		<rdfs:subClassOf rdf:resource="&java;JavaAPI"/>
		<rdfs:comment xml:lang="en">JavaLibrary implementing the javax.security.auth package for Android 1.6</rdfs:comment>
		<rdfs:comment xml:lang="OWLManchester">platform:comprisesInterfacePart some JavaxSecurityAuth</rdfs:comment>
	</owl:Class>
	<owl:Class rdf:about="&android-1_6;JavaxSecurityAuthCallbackAPI">
		<owl:equivalentClass rdf:resource="&android-1_5;JavaxSecurityAuthCallbackAPI"/>
		<rdfs:subClassOf rdf:resource="&java;JavaAPI"/>
		<rdfs:comment xml:lang="en">JavaLibrary implementing the javax.security.auth.callback package for Android 1.6</rdfs:comment>
		<rdfs:comment xml:lang="OWLManchester">platform:comprisesInterfacePart some JavaxSecurityAuthCallback</rdfs:comment>
	</owl:Class>
	<owl:Class rdf:about="&android-1_6;JavaxSecurityAuthX500API">
		<owl:equivalentClass rdf:resource="&android-1_5;JavaxSecurityAuthX500API"/>
		<rdfs:subClassOf rdf:resource="&java;JavaAPI"/>
		<rdfs:comment xml:lang="en">JavaLibrary implementing the javax.security.auth.x500 package for Android 1.6</rdfs:comment>
		<rdfs:comment xml:lang="OWLManchester">platform:comprisesInterfacePart some JavaxSecurityAuthX500</rdfs:comment>
	</owl:Class>
	<owl:Class rdf:about="&android-1_6;JavaxSecurityAuthLoginAPI">
		<owl:equivalentClass rdf:resource="&android-1_5;JavaxSecurityAuthLoginAPI"/>
		<rdfs:subClassOf rdf:resource="&java;JavaAPI"/>
		<rdfs:comment xml:lang="en">JavaLibrary implementing the javax.security.auth.login package for Android 1.6</rdfs:comment>
		<rdfs:comment xml:lang="OWLManchester">platform:comprisesInterfacePart some JavaxSecurityAuthLogin</rdfs:comment>
	</owl:Class>
	<owl:Class rdf:about="&android-1_6;JavaxSecurityCertAPI">
		<owl:equivalentClass rdf:resource="&j2se-5_0;JavaxSecurityCertAPI"/>
		<owl:equivalentClass rdf:resource="&android-1_5;JavaxSecurityCertAPI"/>
		<rdfs:subClassOf rdf:resource="&java;JavaAPI"/>
		<rdfs:comment xml:lang="en">JavaLibrary implementing the javax.security.cert package for Android 1.6</rdfs:comment>
		<rdfs:comment xml:lang="OWLManchester">platform:comprisesInterfacePart some JavaxSecurityCert</rdfs:comment>
	</owl:Class>
	<owl:Class rdf:about="&android-1_6;JavaxCryptoAPI">
		<owl:equivalentClass rdf:resource="&j2se-5_0;JavaxCryptoAPI"/>
		<owl:equivalentClass rdf:resource="&android-1_5;JavaxCryptoAPI"/>
		<rdfs:subClassOf rdf:resource="&java;JavaAPI"/>
		<rdfs:comment xml:lang="en">JavaLibrary implementing the javax.crypto package for Android 1.6</rdfs:comment>
		<rdfs:comment xml:lang="OWLManchester">platform:comprisesInterfacePart some JavaxCrypto</rdfs:comment>
	</owl:Class>
	<owl:Class rdf:about="&android-1_6;JavaxCryptoInterfacesAPI">
		<owl:equivalentClass rdf:resource="&j2se-5_0;JavaxCryptoInterfacesAPI"/>
		<owl:equivalentClass rdf:resource="&android-1_5;JavaxCryptoInterfacesAPI"/>
		<rdfs:subClassOf rdf:resource="&java;JavaAPI"/>
		<rdfs:comment xml:lang="en">JavaLibrary implementing the javax.crypto.interfaces package for Android 1.6</rdfs:comment>
		<rdfs:comment xml:lang="OWLManchester">platform:comprisesInterfacePart some JavaxCryptoInterfaces</rdfs:comment>
	</owl:Class>
	<owl:Class rdf:about="&android-1_6;JavaxCryptoSpecAPI">
		<owl:equivalentClass rdf:resource="&j2se-5_0;JavaxCryptoSpecAPI"/>
		<owl:equivalentClass rdf:resource="&android-1_5;JavaxCryptoSpecAPI"/>
		<rdfs:subClassOf rdf:resource="&java;JavaAPI"/>
		<rdfs:comment xml:lang="en">JavaLibrary implementing the javax.crypto.spec package for Android 1.6</rdfs:comment>
		<rdfs:comment xml:lang="OWLManchester">platform:comprisesInterfacePart some JavaxCryptoSpec</rdfs:comment>
	</owl:Class>
	<owl:Class rdf:about="&android-1_6;JavaxSqlAPI">
		<owl:equivalentClass rdf:resource="&android-1_5;JavaxSqlAPI"/>
		<rdfs:subClassOf rdf:resource="&java;JavaAPI"/>
		<rdfs:comment xml:lang="en">JavaLibrary implementing the javax.sql package for Android 1.6</rdfs:comment>
		<rdfs:comment xml:lang="OWLManchester">platform:comprisesInterfacePart some JavaxSql</rdfs:comment>
	</owl:Class>
	<owl:Class rdf:about="&android-1_6;JavaxXmlAPI">
		<owl:equivalentClass rdf:resource="&android-1_5;JavaxXmlAPI"/>
		<rdfs:subClassOf rdf:resource="&j2se-5_0;JavaxXmlAPI"/>
		<rdfs:comment xml:lang="en">JavaLibrary implementing the javax.xml package for Android 1.6</rdfs:comment>
		<rdfs:comment xml:lang="OWLManchester">platform:comprisesInterfacePart some JavaxXml</rdfs:comment>
	</owl:Class>
	<owl:Class rdf:about="&android-1_6;JavaxXmlParsersAPI">
		<owl:equivalentClass rdf:resource="&android-1_5;JavaxXmlParsersAPI"/>
		<rdfs:subClassOf rdf:resource="&java;JavaAPI"/>
		<rdfs:comment xml:lang="en">JavaLibrary implementing the javax.xml.parsers package for Android 1.6</rdfs:comment>
		<rdfs:comment xml:lang="OWLManchester">platform:comprisesInterfacePart some JavaxXmlParsers</rdfs:comment>
	</owl:Class>
	<owl:Class rdf:about="&android-1_6;JunitFrameworkAPI">
		<owl:equivalentClass rdf:resource="&android-1_5;JunitFrameworkAPI"/>
		<rdfs:subClassOf rdf:resource="&java;JavaAPI"/>
		<rdfs:comment xml:lang="en">JavaLibrary implementing the junit.framework package for Android 1.6</rdfs:comment>
		<rdfs:comment xml:lang="OWLManchester">platform:comprisesInterfacePart some JunitFramework</rdfs:comment>
	</owl:Class>
	<owl:Class rdf:about="&android-1_6;JunitRunnerAPI">
		<owl:equivalentClass rdf:resource="&android-1_5;JunitRunnerAPI"/>
		<rdfs:subClassOf rdf:resource="&java;JavaAPI"/>
		<rdfs:comment xml:lang="en">JavaLibrary implementing the junit.runner package for Android 1.6</rdfs:comment>
		<rdfs:comment xml:lang="OWLManchester">platform:comprisesInterfacePart some JunitRunner</rdfs:comment>
	</owl:Class>
	<owl:Class rdf:about="&android-1_6;DalvikAnnotationAPI">
		<owl:equivalentClass rdf:resource="&android-1_5;DalvikAnnotationAPI"/>
		<rdfs:subClassOf rdf:resource="&java;JavaAPI"/>
		<rdfs:comment xml:lang="en">JavaLibrary implementing the dalvik.annotation package for Android 1.6</rdfs:comment>
		<rdfs:comment xml:lang="OWLManchester">platform:comprisesInterfacePart some DalvikAnnotation</rdfs:comment>
	</owl:Class>
	<owl:Class rdf:about="&android-1_6;DalvikBytecodeAPI">
		<owl:equivalentClass rdf:resource="&android-1_5;DalvikBytecodeAPI"/>
		<rdfs:subClassOf rdf:resource="&java;JavaAPI"/>
		<rdfs:comment xml:lang="en">JavaLibrary implementing the dalvik.bytecode package for Android 1.6</rdfs:comment>
		<rdfs:comment xml:lang="OWLManchester">platform:comprisesInterfacePart some DalvikBytecode</rdfs:comment>
	</owl:Class>
	<owl:Class rdf:about="&android-1_6;DalvikSystemAPI">
		<owl:equivalentClass rdf:resource="&android-1_5;DalvikSystemAPI"/>
		<rdfs:subClassOf rdf:resource="&java;JavaAPI"/>
		<rdfs:comment xml:lang="en">JavaLibrary implementing the dalvik.system package for Android 1.6</rdfs:comment>
		<rdfs:comment xml:lang="OWLManchester">platform:comprisesInterfacePart some DalvikSystem</rdfs:comment>
	</owl:Class>
	<android-1_6:Android rdf:about="&android-1_6;theAndroidPart">
	</android-1_6:Android>
	<android-1_6:AndroidAccessibilityservice rdf:about="&android-1_6;theAndroidAccessibilityservicePart">
	</android-1_6:AndroidAccessibilityservice>
	<android-1_6:AndroidApp rdf:about="&android-1_6;theAndroidAppPart">
	</android-1_6:AndroidApp>
	<android-1_6:AndroidView rdf:about="&android-1_6;theAndroidViewPart">
	</android-1_6:AndroidView>
	<android-1_6:AndroidViewAccessibility rdf:about="&android-1_6;theAndroidViewAccessibilityPart">
	</android-1_6:AndroidViewAccessibility>
	<android-1_6:AndroidViewInputmethod rdf:about="&android-1_6;theAndroidViewInputmethodPart">
	</android-1_6:AndroidViewInputmethod>
	<android-1_6:AndroidViewAnimation rdf:about="&android-1_6;theAndroidViewAnimationPart">
	</android-1_6:AndroidViewAnimation>
	<android-1_6:AndroidContent rdf:about="&android-1_6;theAndroidContentPart">
	</android-1_6:AndroidContent>
	<android-1_6:AndroidContentRes rdf:about="&android-1_6;theAndroidContentResPart">
	</android-1_6:AndroidContentRes>
	<android-1_6:AndroidContentPm rdf:about="&android-1_6;theAndroidContentPmPart">
	</android-1_6:AndroidContentPm>
	<android-1_6:AndroidOs rdf:about="&android-1_6;theAndroidOsPart">
	</android-1_6:AndroidOs>
	<android-1_6:AndroidGraphics rdf:about="&android-1_6;theAndroidGraphicsPart">
	</android-1_6:AndroidGraphics>
	<android-1_6:AndroidGraphicsDrawable rdf:about="&android-1_6;theAndroidGraphicsDrawablePart">
	</android-1_6:AndroidGraphicsDrawable>
	<android-1_6:AndroidGraphicsDrawableShapes rdf:about="&android-1_6;theAndroidGraphicsDrawableShapesPart">
	</android-1_6:AndroidGraphicsDrawableShapes>
	<android-1_6:AndroidNet rdf:about="&android-1_6;theAndroidNetPart">
	</android-1_6:AndroidNet>
	<android-1_6:AndroidNetHttp rdf:about="&android-1_6;theAndroidNetHttpPart">
	</android-1_6:AndroidNetHttp>
	<android-1_6:AndroidNetWifi rdf:about="&android-1_6;theAndroidNetWifiPart">
	</android-1_6:AndroidNetWifi>
	<android-1_6:AndroidDatabase rdf:about="&android-1_6;theAndroidDatabasePart">
	</android-1_6:AndroidDatabase>
	<android-1_6:AndroidDatabaseSqlite rdf:about="&android-1_6;theAndroidDatabaseSqlitePart">
	</android-1_6:AndroidDatabaseSqlite>
	<android-1_6:AndroidUtil rdf:about="&android-1_6;theAndroidUtilPart">
	</android-1_6:AndroidUtil>
	<android-1_6:AndroidWidget rdf:about="&android-1_6;theAndroidWidgetPart">
	</android-1_6:AndroidWidget>
	<android-1_6:AndroidAppwidget rdf:about="&android-1_6;theAndroidAppwidgetPart">
	</android-1_6:AndroidAppwidget>
	<android-1_6:AndroidGesture rdf:about="&android-1_6;theAndroidGesturePart">
	</android-1_6:AndroidGesture>
	<android-1_6:AndroidHardware rdf:about="&android-1_6;theAndroidHardwarePart">
	</android-1_6:AndroidHardware>
	<android-1_6:AndroidInputmethodservice rdf:about="&android-1_6;theAndroidInputmethodservicePart">
	</android-1_6:AndroidInputmethodservice>
	<android-1_6:AndroidLocation rdf:about="&android-1_6;theAndroidLocationPart">
	</android-1_6:AndroidLocation>
	<android-1_6:AndroidMedia rdf:about="&android-1_6;theAndroidMediaPart">
	</android-1_6:AndroidMedia>
	<android-1_6:AndroidOpengl rdf:about="&android-1_6;theAndroidOpenglPart">
	</android-1_6:AndroidOpengl>
	<android-1_6:AndroidPreference rdf:about="&android-1_6;theAndroidPreferencePart">
	</android-1_6:AndroidPreference>
	<android-1_6:AndroidProvider rdf:about="&android-1_6;theAndroidProviderPart">
	</android-1_6:AndroidProvider>
	<android-1_6:AndroidWebkit rdf:about="&android-1_6;theAndroidWebkitPart">
	</android-1_6:AndroidWebkit>
	<android-1_6:AndroidSax rdf:about="&android-1_6;theAndroidSaxPart">
	</android-1_6:AndroidSax>
	<android-1_6:AndroidSpeech rdf:about="&android-1_6;theAndroidSpeechPart">
	</android-1_6:AndroidSpeech>
	<android-1_6:AndroidSpeechTts rdf:about="&android-1_6;theAndroidSpeechTtsPart">
	</android-1_6:AndroidSpeechTts>
	<android-1_6:AndroidTelephony rdf:about="&android-1_6;theAndroidTelephonyPart">
	</android-1_6:AndroidTelephony>
	<android-1_6:AndroidTelephonyGsm rdf:about="&android-1_6;theAndroidTelephonyGsmPart">
	</android-1_6:AndroidTelephonyGsm>
	<android-1_6:AndroidText rdf:about="&android-1_6;theAndroidTextPart">
	</android-1_6:AndroidText>
	<android-1_6:AndroidTextFormat rdf:about="&android-1_6;theAndroidTextFormatPart">
	</android-1_6:AndroidTextFormat>
	<android-1_6:AndroidTextMethod rdf:about="&android-1_6;theAndroidTextMethodPart">
	</android-1_6:AndroidTextMethod>
	<android-1_6:AndroidTextStyle rdf:about="&android-1_6;theAndroidTextStylePart">
	</android-1_6:AndroidTextStyle>
	<android-1_6:AndroidTextUtil rdf:about="&android-1_6;theAndroidTextUtilPart">
	</android-1_6:AndroidTextUtil>
	<android-1_6:AndroidTest rdf:about="&android-1_6;theAndroidTestPart">
	</android-1_6:AndroidTest>
	<android-1_6:AndroidTestMock rdf:about="&android-1_6;theAndroidTestMockPart">
	</android-1_6:AndroidTestMock>
	<android-1_6:AndroidTestSuitebuilder rdf:about="&android-1_6;theAndroidTestSuitebuilderPart">
	</android-1_6:AndroidTestSuitebuilder>
	<android-1_6:AndroidTestSuitebuilderAnnotation rdf:about="&android-1_6;theAndroidTestSuitebuilderAnnotationPart">
	</android-1_6:AndroidTestSuitebuilderAnnotation>
	<android-1_6:JavaLang rdf:about="&android-1_6;theJavaLangPart">
	</android-1_6:JavaLang>
	<android-1_6:JavaLangAnnotation rdf:about="&android-1_6;theJavaLangAnnotationPart">
	</android-1_6:JavaLangAnnotation>
	<android-1_6:JavaLangReflect rdf:about="&android-1_6;theJavaLangReflectPart">
	</android-1_6:JavaLangReflect>
	<android-1_6:JavaLangRef rdf:about="&android-1_6;theJavaLangRefPart">
	</android-1_6:JavaLangRef>
	<android-1_6:JavaUtil rdf:about="&android-1_6;theJavaUtilPart">
	</android-1_6:JavaUtil>
	<android-1_6:JavaUtilConcurrent rdf:about="&android-1_6;theJavaUtilConcurrentPart">
	</android-1_6:JavaUtilConcurrent>
	<android-1_6:JavaUtilConcurrentAtomic rdf:about="&android-1_6;theJavaUtilConcurrentAtomicPart">
	</android-1_6:JavaUtilConcurrentAtomic>
	<android-1_6:JavaUtilConcurrentLocks rdf:about="&android-1_6;theJavaUtilConcurrentLocksPart">
	</android-1_6:JavaUtilConcurrentLocks>
	<android-1_6:JavaUtilRegex rdf:about="&android-1_6;theJavaUtilRegexPart">
	</android-1_6:JavaUtilRegex>
	<android-1_6:JavaUtilJar rdf:about="&android-1_6;theJavaUtilJarPart">
	</android-1_6:JavaUtilJar>
	<android-1_6:JavaUtilZip rdf:about="&android-1_6;theJavaUtilZipPart">
	</android-1_6:JavaUtilZip>
	<android-1_6:JavaUtilLogging rdf:about="&android-1_6;theJavaUtilLoggingPart">
	</android-1_6:JavaUtilLogging>
	<android-1_6:JavaUtilPrefs rdf:about="&android-1_6;theJavaUtilPrefsPart">
	</android-1_6:JavaUtilPrefs>
	<android-1_6:JavaIo rdf:about="&android-1_6;theJavaIoPart">
	</android-1_6:JavaIo>
	<android-1_6:JavaNio rdf:about="&android-1_6;theJavaNioPart">
	</android-1_6:JavaNio>
	<android-1_6:JavaNioChannels rdf:about="&android-1_6;theJavaNioChannelsPart">
	</android-1_6:JavaNioChannels>
	<android-1_6:JavaNioChannelsSpi rdf:about="&android-1_6;theJavaNioChannelsSpiPart">
	</android-1_6:JavaNioChannelsSpi>
	<android-1_6:JavaNioCharset rdf:about="&android-1_6;theJavaNioCharsetPart">
	</android-1_6:JavaNioCharset>
	<android-1_6:JavaNioCharsetSpi rdf:about="&android-1_6;theJavaNioCharsetSpiPart">
	</android-1_6:JavaNioCharsetSpi>
	<android-1_6:JavaNet rdf:about="&android-1_6;theJavaNetPart">
	</android-1_6:JavaNet>
	<android-1_6:JavaSecurity rdf:about="&android-1_6;theJavaSecurityPart">
	</android-1_6:JavaSecurity>
	<android-1_6:JavaSecurityCert rdf:about="&android-1_6;theJavaSecurityCertPart">
	</android-1_6:JavaSecurityCert>
	<android-1_6:JavaSecuritySpec rdf:about="&android-1_6;theJavaSecuritySpecPart">
	</android-1_6:JavaSecuritySpec>
	<android-1_6:JavaSecurityAcl rdf:about="&android-1_6;theJavaSecurityAclPart">
	</android-1_6:JavaSecurityAcl>
	<android-1_6:JavaSecurityInterfaces rdf:about="&android-1_6;theJavaSecurityInterfacesPart">
	</android-1_6:JavaSecurityInterfaces>
	<android-1_6:JavaText rdf:about="&android-1_6;theJavaTextPart">
	</android-1_6:JavaText>
	<android-1_6:JavaAwtFont rdf:about="&android-1_6;theJavaAwtFontPart">
	</android-1_6:JavaAwtFont>
	<android-1_6:JavaBeans rdf:about="&android-1_6;theJavaBeansPart">
	</android-1_6:JavaBeans>
	<android-1_6:JavaMath rdf:about="&android-1_6;theJavaMathPart">
	</android-1_6:JavaMath>
	<android-1_6:JavaSql rdf:about="&android-1_6;theJavaSqlPart">
	</android-1_6:JavaSql>
	<android-1_6:OrgXmlpullV1 rdf:about="&android-1_6;theOrgXmlpullV1Part">
	</android-1_6:OrgXmlpullV1>
	<android-1_6:OrgXmlpullV1Sax2 rdf:about="&android-1_6;theOrgXmlpullV1Sax2Part">
	</android-1_6:OrgXmlpullV1Sax2>
	<android-1_6:OrgXmlSax rdf:about="&android-1_6;theOrgXmlSaxPart">
	</android-1_6:OrgXmlSax>
	<android-1_6:OrgXmlSaxHelpers rdf:about="&android-1_6;theOrgXmlSaxHelpersPart">
	</android-1_6:OrgXmlSaxHelpers>
	<android-1_6:OrgXmlSaxExt rdf:about="&android-1_6;theOrgXmlSaxExtPart">
	</android-1_6:OrgXmlSaxExt>
	<android-1_6:OrgW3cDom rdf:about="&android-1_6;theOrgW3cDomPart">
	</android-1_6:OrgW3cDom>
	<android-1_6:OrgApacheCommonsLogging rdf:about="&android-1_6;theOrgApacheCommonsLoggingPart">
	</android-1_6:OrgApacheCommonsLogging>
	<android-1_6:OrgApacheHttp rdf:about="&android-1_6;theOrgApacheHttpPart">
	</android-1_6:OrgApacheHttp>
	<android-1_6:OrgApacheHttpProtocol rdf:about="&android-1_6;theOrgApacheHttpProtocolPart">
	</android-1_6:OrgApacheHttpProtocol>
	<android-1_6:OrgApacheHttpUtil rdf:about="&android-1_6;theOrgApacheHttpUtilPart">
	</android-1_6:OrgApacheHttpUtil>
	<android-1_6:OrgApacheHttpParams rdf:about="&android-1_6;theOrgApacheHttpParamsPart">
	</android-1_6:OrgApacheHttpParams>
	<android-1_6:OrgApacheHttpAuth rdf:about="&android-1_6;theOrgApacheHttpAuthPart">
	</android-1_6:OrgApacheHttpAuth>
	<android-1_6:OrgApacheHttpAuthParams rdf:about="&android-1_6;theOrgApacheHttpAuthParamsPart">
	</android-1_6:OrgApacheHttpAuthParams>
	<android-1_6:OrgApacheHttpClient rdf:about="&android-1_6;theOrgApacheHttpClientPart">
	</android-1_6:OrgApacheHttpClient>
	<android-1_6:OrgApacheHttpClientMethods rdf:about="&android-1_6;theOrgApacheHttpClientMethodsPart">
	</android-1_6:OrgApacheHttpClientMethods>
	<android-1_6:OrgApacheHttpClientEntity rdf:about="&android-1_6;theOrgApacheHttpClientEntityPart">
	</android-1_6:OrgApacheHttpClientEntity>
	<android-1_6:OrgApacheHttpClientParams rdf:about="&android-1_6;theOrgApacheHttpClientParamsPart">
	</android-1_6:OrgApacheHttpClientParams>
	<android-1_6:OrgApacheHttpClientProtocol rdf:about="&android-1_6;theOrgApacheHttpClientProtocolPart">
	</android-1_6:OrgApacheHttpClientProtocol>
	<android-1_6:OrgApacheHttpClientUtils rdf:about="&android-1_6;theOrgApacheHttpClientUtilsPart">
	</android-1_6:OrgApacheHttpClientUtils>
	<android-1_6:OrgApacheHttpCookie rdf:about="&android-1_6;theOrgApacheHttpCookiePart">
	</android-1_6:OrgApacheHttpCookie>
	<android-1_6:OrgApacheHttpCookieParams rdf:about="&android-1_6;theOrgApacheHttpCookieParamsPart">
	</android-1_6:OrgApacheHttpCookieParams>
	<android-1_6:OrgApacheHttpConn rdf:about="&android-1_6;theOrgApacheHttpConnPart">
	</android-1_6:OrgApacheHttpConn>
	<android-1_6:OrgApacheHttpConnParams rdf:about="&android-1_6;theOrgApacheHttpConnParamsPart">
	</android-1_6:OrgApacheHttpConnParams>
	<android-1_6:OrgApacheHttpConnScheme rdf:about="&android-1_6;theOrgApacheHttpConnSchemePart">
	</android-1_6:OrgApacheHttpConnScheme>
	<android-1_6:OrgApacheHttpConnRouting rdf:about="&android-1_6;theOrgApacheHttpConnRoutingPart">
	</android-1_6:OrgApacheHttpConnRouting>
	<android-1_6:OrgApacheHttpConnSsl rdf:about="&android-1_6;theOrgApacheHttpConnSslPart">
	</android-1_6:OrgApacheHttpConnSsl>
	<android-1_6:OrgApacheHttpConnUtil rdf:about="&android-1_6;theOrgApacheHttpConnUtilPart">
	</android-1_6:OrgApacheHttpConnUtil>
	<android-1_6:OrgApacheHttpEntity rdf:about="&android-1_6;theOrgApacheHttpEntityPart">
	</android-1_6:OrgApacheHttpEntity>
	<android-1_6:OrgApacheHttpMessage rdf:about="&android-1_6;theOrgApacheHttpMessagePart">
	</android-1_6:OrgApacheHttpMessage>
	<android-1_6:OrgApacheHttpImpl rdf:about="&android-1_6;theOrgApacheHttpImplPart">
	</android-1_6:OrgApacheHttpImpl>
	<android-1_6:OrgApacheHttpImplEntity rdf:about="&android-1_6;theOrgApacheHttpImplEntityPart">
	</android-1_6:OrgApacheHttpImplEntity>
	<android-1_6:OrgApacheHttpImplAuth rdf:about="&android-1_6;theOrgApacheHttpImplAuthPart">
	</android-1_6:OrgApacheHttpImplAuth>
	<android-1_6:OrgApacheHttpImplClient rdf:about="&android-1_6;theOrgApacheHttpImplClientPart">
	</android-1_6:OrgApacheHttpImplClient>
	<android-1_6:OrgApacheHttpImplConn rdf:about="&android-1_6;theOrgApacheHttpImplConnPart">
	</android-1_6:OrgApacheHttpImplConn>
	<android-1_6:OrgApacheHttpImplConnTsccm rdf:about="&android-1_6;theOrgApacheHttpImplConnTsccmPart">
	</android-1_6:OrgApacheHttpImplConnTsccm>
	<android-1_6:OrgApacheHttpImplIo rdf:about="&android-1_6;theOrgApacheHttpImplIoPart">
	</android-1_6:OrgApacheHttpImplIo>
	<android-1_6:OrgApacheHttpImplCookie rdf:about="&android-1_6;theOrgApacheHttpImplCookiePart">
	</android-1_6:OrgApacheHttpImplCookie>
	<android-1_6:OrgApacheHttpIo rdf:about="&android-1_6;theOrgApacheHttpIoPart">
	</android-1_6:OrgApacheHttpIo>
	<android-1_6:OrgJson rdf:about="&android-1_6;theOrgJsonPart">
	</android-1_6:OrgJson>
	<android-1_6:JavaxMicroeditionKhronosOpengles rdf:about="&android-1_6;theJavaxMicroeditionKhronosOpenglesPart">
	</android-1_6:JavaxMicroeditionKhronosOpengles>
	<android-1_6:JavaxMicroeditionKhronosEgl rdf:about="&android-1_6;theJavaxMicroeditionKhronosEglPart">
	</android-1_6:JavaxMicroeditionKhronosEgl>
	<android-1_6:JavaxNet rdf:about="&android-1_6;theJavaxNetPart">
	</android-1_6:JavaxNet>
	<android-1_6:JavaxNetSsl rdf:about="&android-1_6;theJavaxNetSslPart">
	</android-1_6:JavaxNetSsl>
	<android-1_6:JavaxSecurityAuth rdf:about="&android-1_6;theJavaxSecurityAuthPart">
	</android-1_6:JavaxSecurityAuth>
	<android-1_6:JavaxSecurityAuthCallback rdf:about="&android-1_6;theJavaxSecurityAuthCallbackPart">
	</android-1_6:JavaxSecurityAuthCallback>
	<android-1_6:JavaxSecurityAuthX500 rdf:about="&android-1_6;theJavaxSecurityAuthX500Part">
	</android-1_6:JavaxSecurityAuthX500>
	<android-1_6:JavaxSecurityAuthLogin rdf:about="&android-1_6;theJavaxSecurityAuthLoginPart">
	</android-1_6:JavaxSecurityAuthLogin>
	<android-1_6:JavaxSecurityCert rdf:about="&android-1_6;theJavaxSecurityCertPart">
	</android-1_6:JavaxSecurityCert>
	<android-1_6:JavaxCrypto rdf:about="&android-1_6;theJavaxCryptoPart">
	</android-1_6:JavaxCrypto>
	<android-1_6:JavaxCryptoInterfaces rdf:about="&android-1_6;theJavaxCryptoInterfacesPart">
	</android-1_6:JavaxCryptoInterfaces>
	<android-1_6:JavaxCryptoSpec rdf:about="&android-1_6;theJavaxCryptoSpecPart">
	</android-1_6:JavaxCryptoSpec>
	<android-1_6:JavaxSql rdf:about="&android-1_6;theJavaxSqlPart">
	</android-1_6:JavaxSql>
	<android-1_6:JavaxXml rdf:about="&android-1_6;theJavaxXmlPart">
	</android-1_6:JavaxXml>
	<android-1_6:JavaxXmlParsers rdf:about="&android-1_6;theJavaxXmlParsersPart">
	</android-1_6:JavaxXmlParsers>
	<android-1_6:JunitFramework rdf:about="&android-1_6;theJunitFrameworkPart">
	</android-1_6:JunitFramework>
	<android-1_6:JunitRunner rdf:about="&android-1_6;theJunitRunnerPart">
	</android-1_6:JunitRunner>
	<android-1_6:DalvikAnnotation rdf:about="&android-1_6;theDalvikAnnotationPart">
	</android-1_6:DalvikAnnotation>
	<android-1_6:DalvikBytecode rdf:about="&android-1_6;theDalvikBytecodePart">
	</android-1_6:DalvikBytecode>
	<android-1_6:DalvikSystem rdf:about="&android-1_6;theDalvikSystemPart">
	</android-1_6:DalvikSystem>
	<owl:Class rdf:about="&android-1_6;AndroidClassLibrary">
		<rdfs:subClassOf rdf:resource="&java;JavaClassLibrary"/>
		<rdfs:comment xml:lang="en">JavaLibrary implementing the android package for Android 1.6</rdfs:comment>
		<rdfs:comment xml:lang="OWLManchester">platform:implementsInterface some AndroidAPI</rdfs:comment>
	</owl:Class>
	<owl:Class rdf:about="&android-1_6;AndroidAccessibilityserviceClassLibrary">
		<rdfs:subClassOf rdf:resource="&java;JavaClassLibrary"/>
		<rdfs:comment xml:lang="en">JavaLibrary implementing the android.accessibilityservice package for Android 1.6</rdfs:comment>
		<rdfs:comment xml:lang="OWLManchester">platform:implementsInterface some AndroidAccessibilityserviceAPI</rdfs:comment>
	</owl:Class>
	<owl:Class rdf:about="&android-1_6;AndroidAppClassLibrary">
		<rdfs:subClassOf rdf:resource="&android-1_5;AndroidAppClassLibrary"/>
		<rdfs:comment xml:lang="en">JavaLibrary implementing the android.app package for Android 1.6</rdfs:comment>
		<rdfs:comment xml:lang="OWLManchester">platform:implementsInterface some AndroidAppAPI</rdfs:comment>
	</owl:Class>
	<owl:Class rdf:about="&android-1_6;AndroidViewClassLibrary">
		<rdfs:subClassOf rdf:resource="&android-1_5;AndroidViewClassLibrary"/>
		<rdfs:comment xml:lang="en">JavaLibrary implementing the android.view package for Android 1.6</rdfs:comment>
		<rdfs:comment xml:lang="OWLManchester">platform:implementsInterface some AndroidViewAPI</rdfs:comment>
	</owl:Class>
	<owl:Class rdf:about="&android-1_6;AndroidViewAccessibilityClassLibrary">
		<rdfs:subClassOf rdf:resource="&java;JavaClassLibrary"/>
		<rdfs:comment xml:lang="en">JavaLibrary implementing the android.view.accessibility package for Android 1.6</rdfs:comment>
		<rdfs:comment xml:lang="OWLManchester">platform:implementsInterface some AndroidViewAccessibilityAPI</rdfs:comment>
	</owl:Class>
	<owl:Class rdf:about="&android-1_6;AndroidViewInputmethodClassLibrary">
		<owl:equivalentClass rdf:resource="&android-1_5;AndroidViewInputmethodClassLibrary"/>
		<rdfs:subClassOf rdf:resource="&java;JavaClassLibrary"/>
		<rdfs:comment xml:lang="en">JavaLibrary implementing the android.view.inputmethod package for Android 1.6</rdfs:comment>
		<rdfs:comment xml:lang="OWLManchester">platform:implementsInterface some AndroidViewInputmethodAPI</rdfs:comment>
	</owl:Class>
	<owl:Class rdf:about="&android-1_6;AndroidViewAnimationClassLibrary">
		<rdfs:subClassOf rdf:resource="&android-1_5;AndroidViewAnimationClassLibrary"/>
		<rdfs:comment xml:lang="en">JavaLibrary implementing the android.view.animation package for Android 1.6</rdfs:comment>
		<rdfs:comment xml:lang="OWLManchester">platform:implementsInterface some AndroidViewAnimationAPI</rdfs:comment>
	</owl:Class>
	<owl:Class rdf:about="&android-1_6;AndroidContentClassLibrary">
		<rdfs:subClassOf rdf:resource="&android-1_5;AndroidContentClassLibrary"/>
		<rdfs:comment xml:lang="en">JavaLibrary implementing the android.content package for Android 1.6</rdfs:comment>
		<rdfs:comment xml:lang="OWLManchester">platform:implementsInterface some AndroidContentAPI</rdfs:comment>
	</owl:Class>
	<owl:Class rdf:about="&android-1_6;AndroidContentResClassLibrary">
		<rdfs:subClassOf rdf:resource="&android-1_5;AndroidContentResClassLibrary"/>
		<rdfs:comment xml:lang="en">JavaLibrary implementing the android.content.res package for Android 1.6</rdfs:comment>
		<rdfs:comment xml:lang="OWLManchester">platform:implementsInterface some AndroidContentResAPI</rdfs:comment>
	</owl:Class>
	<owl:Class rdf:about="&android-1_6;AndroidContentPmClassLibrary">
		<rdfs:subClassOf rdf:resource="&java;JavaClassLibrary"/>
		<rdfs:comment xml:lang="en">JavaLibrary implementing the android.content.pm package for Android 1.6</rdfs:comment>
		<rdfs:comment xml:lang="OWLManchester">platform:implementsInterface some AndroidContentPmAPI</rdfs:comment>
	</owl:Class>
	<owl:Class rdf:about="&android-1_6;AndroidOsClassLibrary">
		<rdfs:subClassOf rdf:resource="&android-1_5;AndroidOsClassLibrary"/>
		<rdfs:comment xml:lang="en">JavaLibrary implementing the android.os package for Android 1.6</rdfs:comment>
		<rdfs:comment xml:lang="OWLManchester">platform:implementsInterface some AndroidOsAPI</rdfs:comment>
	</owl:Class>
	<owl:Class rdf:about="&android-1_6;AndroidGraphicsClassLibrary">
		<rdfs:subClassOf rdf:resource="&android-1_5;AndroidGraphicsClassLibrary"/>
		<rdfs:comment xml:lang="en">JavaLibrary implementing the android.graphics package for Android 1.6</rdfs:comment>
		<rdfs:comment xml:lang="OWLManchester">platform:implementsInterface some AndroidGraphicsAPI</rdfs:comment>
	</owl:Class>
	<owl:Class rdf:about="&android-1_6;AndroidGraphicsDrawableClassLibrary">
		<rdfs:subClassOf rdf:resource="&android-1_5;AndroidGraphicsDrawableClassLibrary"/>
		<rdfs:comment xml:lang="en">JavaLibrary implementing the android.graphics.drawable package for Android 1.6</rdfs:comment>
		<rdfs:comment xml:lang="OWLManchester">platform:implementsInterface some AndroidGraphicsDrawableAPI</rdfs:comment>
	</owl:Class>
	<owl:Class rdf:about="&android-1_6;AndroidGraphicsDrawableShapesClassLibrary">
		<owl:equivalentClass rdf:resource="&android-1_5;AndroidGraphicsDrawableShapesClassLibrary"/>
		<rdfs:subClassOf rdf:resource="&java;JavaClassLibrary"/>
		<rdfs:comment xml:lang="en">JavaLibrary implementing the android.graphics.drawable.shapes package for Android 1.6</rdfs:comment>
		<rdfs:comment xml:lang="OWLManchester">platform:implementsInterface some AndroidGraphicsDrawableShapesAPI</rdfs:comment>
	</owl:Class>
	<owl:Class rdf:about="&android-1_6;AndroidNetClassLibrary">
		<owl:equivalentClass rdf:resource="&android-1_5;AndroidNetClassLibrary"/>
		<rdfs:subClassOf rdf:resource="&java;JavaClassLibrary"/>
		<rdfs:comment xml:lang="en">JavaLibrary implementing the android.net package for Android 1.6</rdfs:comment>
		<rdfs:comment xml:lang="OWLManchester">platform:implementsInterface some AndroidNetAPI</rdfs:comment>
	</owl:Class>
	<owl:Class rdf:about="&android-1_6;AndroidNetHttpClassLibrary">
		<owl:equivalentClass rdf:resource="&android-1_5;AndroidNetHttpClassLibrary"/>
		<rdfs:subClassOf rdf:resource="&java;JavaClassLibrary"/>
		<rdfs:comment xml:lang="en">JavaLibrary implementing the android.net.http package for Android 1.6</rdfs:comment>
		<rdfs:comment xml:lang="OWLManchester">platform:implementsInterface some AndroidNetHttpAPI</rdfs:comment>
	</owl:Class>
	<owl:Class rdf:about="&android-1_6;AndroidNetWifiClassLibrary">
		<rdfs:subClassOf rdf:resource="&android-1_5;AndroidNetWifiClassLibrary"/>
		<rdfs:comment xml:lang="en">JavaLibrary implementing the android.net.wifi package for Android 1.6</rdfs:comment>
		<rdfs:comment xml:lang="OWLManchester">platform:implementsInterface some AndroidNetWifiAPI</rdfs:comment>
	</owl:Class>
	<owl:Class rdf:about="&android-1_6;AndroidDatabaseClassLibrary">
		<owl:equivalentClass rdf:resource="&android-1_5;AndroidDatabaseClassLibrary"/>
		<rdfs:subClassOf rdf:resource="&java;JavaClassLibrary"/>
		<rdfs:comment xml:lang="en">JavaLibrary implementing the android.database package for Android 1.6</rdfs:comment>
		<rdfs:comment xml:lang="OWLManchester">platform:implementsInterface some AndroidDatabaseAPI</rdfs:comment>
	</owl:Class>
	<owl:Class rdf:about="&android-1_6;AndroidDatabaseSqliteClassLibrary">
		<owl:equivalentClass rdf:resource="&android-1_5;AndroidDatabaseSqliteClassLibrary"/>
		<rdfs:subClassOf rdf:resource="&java;JavaClassLibrary"/>
		<rdfs:comment xml:lang="en">JavaLibrary implementing the android.database.sqlite package for Android 1.6</rdfs:comment>
		<rdfs:comment xml:lang="OWLManchester">platform:implementsInterface some AndroidDatabaseSqliteAPI</rdfs:comment>
	</owl:Class>
	<owl:Class rdf:about="&android-1_6;AndroidUtilClassLibrary">
		<rdfs:subClassOf rdf:resource="&android-1_5;AndroidUtilClassLibrary"/>
		<rdfs:comment xml:lang="en">JavaLibrary implementing the android.util package for Android 1.6</rdfs:comment>
		<rdfs:comment xml:lang="OWLManchester">platform:implementsInterface some AndroidUtilAPI</rdfs:comment>
	</owl:Class>
	<owl:Class rdf:about="&android-1_6;AndroidWidgetClassLibrary">
		<rdfs:subClassOf rdf:resource="&android-1_5;AndroidWidgetClassLibrary"/>
		<rdfs:comment xml:lang="en">JavaLibrary implementing the android.widget package for Android 1.6</rdfs:comment>
		<rdfs:comment xml:lang="OWLManchester">platform:implementsInterface some AndroidWidgetAPI</rdfs:comment>
	</owl:Class>
	<owl:Class rdf:about="&android-1_6;AndroidAppwidgetClassLibrary">
		<rdfs:subClassOf rdf:resource="&android-1_5;AndroidAppwidgetClassLibrary"/>
		<rdfs:comment xml:lang="en">JavaLibrary implementing the android.appwidget package for Android 1.6</rdfs:comment>
		<rdfs:comment xml:lang="OWLManchester">platform:implementsInterface some AndroidAppwidgetAPI</rdfs:comment>
	</owl:Class>
	<owl:Class rdf:about="&android-1_6;AndroidGestureClassLibrary">
		<rdfs:subClassOf rdf:resource="&java;JavaClassLibrary"/>
		<rdfs:comment xml:lang="en">JavaLibrary implementing the android.gesture package for Android 1.6</rdfs:comment>
		<rdfs:comment xml:lang="OWLManchester">platform:implementsInterface some AndroidGestureAPI</rdfs:comment>
	</owl:Class>
	<owl:Class rdf:about="&android-1_6;AndroidHardwareClassLibrary">
		<owl:equivalentClass rdf:resource="&android-1_5;AndroidHardwareClassLibrary"/>
		<rdfs:subClassOf rdf:resource="&java;JavaClassLibrary"/>
		<rdfs:comment xml:lang="en">JavaLibrary implementing the android.hardware package for Android 1.6</rdfs:comment>
		<rdfs:comment xml:lang="OWLManchester">platform:implementsInterface some AndroidHardwareAPI</rdfs:comment>
	</owl:Class>
	<owl:Class rdf:about="&android-1_6;AndroidInputmethodserviceClassLibrary">
		<rdfs:subClassOf rdf:resource="&android-1_5;AndroidInputmethodserviceClassLibrary"/>
		<rdfs:comment xml:lang="en">JavaLibrary implementing the android.inputmethodservice package for Android 1.6</rdfs:comment>
		<rdfs:comment xml:lang="OWLManchester">platform:implementsInterface some AndroidInputmethodserviceAPI</rdfs:comment>
	</owl:Class>
	<owl:Class rdf:about="&android-1_6;AndroidLocationClassLibrary">
		<rdfs:subClassOf rdf:resource="&android-1_5;AndroidLocationClassLibrary"/>
		<rdfs:comment xml:lang="en">JavaLibrary implementing the android.location package for Android 1.6</rdfs:comment>
		<rdfs:comment xml:lang="OWLManchester">platform:implementsInterface some AndroidLocationAPI</rdfs:comment>
	</owl:Class>
	<owl:Class rdf:about="&android-1_6;AndroidMediaClassLibrary">
		<rdfs:subClassOf rdf:resource="&android-1_5;AndroidMediaClassLibrary"/>
		<rdfs:comment xml:lang="en">JavaLibrary implementing the android.media package for Android 1.6</rdfs:comment>
		<rdfs:comment xml:lang="OWLManchester">platform:implementsInterface some AndroidMediaAPI</rdfs:comment>
	</owl:Class>
	<owl:Class rdf:about="&android-1_6;AndroidOpenglClassLibrary">
		<rdfs:subClassOf rdf:resource="&android-1_5;AndroidOpenglClassLibrary"/>
		<rdfs:comment xml:lang="en">JavaLibrary implementing the android.opengl package for Android 1.6</rdfs:comment>
		<rdfs:comment xml:lang="OWLManchester">platform:implementsInterface some AndroidOpenglAPI</rdfs:comment>
	</owl:Class>
	<owl:Class rdf:about="&android-1_6;AndroidPreferenceClassLibrary">
		<rdfs:subClassOf rdf:resource="&android-1_5;AndroidPreferenceClassLibrary"/>
		<rdfs:comment xml:lang="en">JavaLibrary implementing the android.preference package for Android 1.6</rdfs:comment>
		<rdfs:comment xml:lang="OWLManchester">platform:implementsInterface some AndroidPreferenceAPI</rdfs:comment>
	</owl:Class>
	<owl:Class rdf:about="&android-1_6;AndroidProviderClassLibrary">
		<rdfs:subClassOf rdf:resource="&android-1_5;AndroidProviderClassLibrary"/>
		<rdfs:comment xml:lang="en">JavaLibrary implementing the android.provider package for Android 1.6</rdfs:comment>
		<rdfs:comment xml:lang="OWLManchester">platform:implementsInterface some AndroidProviderAPI</rdfs:comment>
	</owl:Class>
	<owl:Class rdf:about="&android-1_6;AndroidWebkitClassLibrary">
		<rdfs:subClassOf rdf:resource="&android-1_5;AndroidWebkitClassLibrary"/>
		<rdfs:comment xml:lang="en">JavaLibrary implementing the android.webkit package for Android 1.6</rdfs:comment>
		<rdfs:comment xml:lang="OWLManchester">platform:implementsInterface some AndroidWebkitAPI</rdfs:comment>
	</owl:Class>
	<owl:Class rdf:about="&android-1_6;AndroidSaxClassLibrary">
		<owl:equivalentClass rdf:resource="&android-1_5;AndroidSaxClassLibrary"/>
		<rdfs:subClassOf rdf:resource="&java;JavaClassLibrary"/>
		<rdfs:comment xml:lang="en">JavaLibrary implementing the android.sax package for Android 1.6</rdfs:comment>
		<rdfs:comment xml:lang="OWLManchester">platform:implementsInterface some AndroidSaxAPI</rdfs:comment>
	</owl:Class>
	<owl:Class rdf:about="&android-1_6;AndroidSpeechClassLibrary">
		<owl:equivalentClass rdf:resource="&android-1_5;AndroidSpeechClassLibrary"/>
		<rdfs:subClassOf rdf:resource="&java;JavaClassLibrary"/>
		<rdfs:comment xml:lang="en">JavaLibrary implementing the android.speech package for Android 1.6</rdfs:comment>
		<rdfs:comment xml:lang="OWLManchester">platform:implementsInterface some AndroidSpeechAPI</rdfs:comment>
	</owl:Class>
	<owl:Class rdf:about="&android-1_6;AndroidSpeechTtsClassLibrary">
		<rdfs:subClassOf rdf:resource="&java;JavaClassLibrary"/>
		<rdfs:comment xml:lang="en">JavaLibrary implementing the android.speech.tts package for Android 1.6</rdfs:comment>
		<rdfs:comment xml:lang="OWLManchester">platform:implementsInterface some AndroidSpeechTtsAPI</rdfs:comment>
	</owl:Class>
	<owl:Class rdf:about="&android-1_6;AndroidTelephonyClassLibrary">
		<rdfs:subClassOf rdf:resource="&android-1_5;AndroidTelephonyClassLibrary"/>
		<rdfs:comment xml:lang="en">JavaLibrary implementing the android.telephony package for Android 1.6</rdfs:comment>
		<rdfs:comment xml:lang="OWLManchester">platform:implementsInterface some AndroidTelephonyAPI</rdfs:comment>
	</owl:Class>
	<owl:Class rdf:about="&android-1_6;AndroidTelephonyGsmClassLibrary">
		<rdfs:subClassOf rdf:resource="&java;JavaClassLibrary"/>
		<rdfs:comment xml:lang="en">JavaLibrary implementing the android.telephony.gsm package for Android 1.6</rdfs:comment>
		<rdfs:comment xml:lang="OWLManchester">platform:implementsInterface some AndroidTelephonyGsmAPI</rdfs:comment>
	</owl:Class>
	<owl:Class rdf:about="&android-1_6;AndroidTextClassLibrary">
		<owl:equivalentClass rdf:resource="&android-1_5;AndroidTextClassLibrary"/>
		<rdfs:subClassOf rdf:resource="&java;JavaClassLibrary"/>
		<rdfs:comment xml:lang="en">JavaLibrary implementing the android.text package for Android 1.6</rdfs:comment>
		<rdfs:comment xml:lang="OWLManchester">platform:implementsInterface some AndroidTextAPI</rdfs:comment>
	</owl:Class>
	<owl:Class rdf:about="&android-1_6;AndroidTextFormatClassLibrary">
		<owl:equivalentClass rdf:resource="&android-1_5;AndroidTextFormatClassLibrary"/>
		<rdfs:subClassOf rdf:resource="&java;JavaClassLibrary"/>
		<rdfs:comment xml:lang="en">JavaLibrary implementing the android.text.format package for Android 1.6</rdfs:comment>
		<rdfs:comment xml:lang="OWLManchester">platform:implementsInterface some AndroidTextFormatAPI</rdfs:comment>
	</owl:Class>
	<owl:Class rdf:about="&android-1_6;AndroidTextMethodClassLibrary">
		<rdfs:subClassOf rdf:resource="&android-1_5;AndroidTextMethodClassLibrary"/>
		<rdfs:comment xml:lang="en">JavaLibrary implementing the android.text.method package for Android 1.6</rdfs:comment>
		<rdfs:comment xml:lang="OWLManchester">platform:implementsInterface some AndroidTextMethodAPI</rdfs:comment>
	</owl:Class>
	<owl:Class rdf:about="&android-1_6;AndroidTextStyleClassLibrary">
		<rdfs:subClassOf rdf:resource="&android-1_5;AndroidTextStyleClassLibrary"/>
		<rdfs:comment xml:lang="en">JavaLibrary implementing the android.text.style package for Android 1.6</rdfs:comment>
		<rdfs:comment xml:lang="OWLManchester">platform:implementsInterface some AndroidTextStyleAPI</rdfs:comment>
	</owl:Class>
	<owl:Class rdf:about="&android-1_6;AndroidTextUtilClassLibrary">
		<owl:equivalentClass rdf:resource="&android-1_5;AndroidTextUtilClassLibrary"/>
		<rdfs:subClassOf rdf:resource="&java;JavaClassLibrary"/>
		<rdfs:comment xml:lang="en">JavaLibrary implementing the android.text.util package for Android 1.6</rdfs:comment>
		<rdfs:comment xml:lang="OWLManchester">platform:implementsInterface some AndroidTextUtilAPI</rdfs:comment>
	</owl:Class>
	<owl:Class rdf:about="&android-1_6;AndroidTestClassLibrary">
		<rdfs:subClassOf rdf:resource="&android-1_5;AndroidTestClassLibrary"/>
		<rdfs:comment xml:lang="en">JavaLibrary implementing the android.test package for Android 1.6</rdfs:comment>
		<rdfs:comment xml:lang="OWLManchester">platform:implementsInterface some AndroidTestAPI</rdfs:comment>
	</owl:Class>
	<owl:Class rdf:about="&android-1_6;AndroidTestMockClassLibrary">
		<rdfs:subClassOf rdf:resource="&java;JavaClassLibrary"/>
		<rdfs:comment xml:lang="en">JavaLibrary implementing the android.test.mock package for Android 1.6</rdfs:comment>
		<rdfs:comment xml:lang="OWLManchester">platform:implementsInterface some AndroidTestMockAPI</rdfs:comment>
	</owl:Class>
	<owl:Class rdf:about="&android-1_6;AndroidTestSuitebuilderClassLibrary">
		<owl:equivalentClass rdf:resource="&android-1_5;AndroidTestSuitebuilderClassLibrary"/>
		<rdfs:subClassOf rdf:resource="&java;JavaClassLibrary"/>
		<rdfs:comment xml:lang="en">JavaLibrary implementing the android.test.suitebuilder package for Android 1.6</rdfs:comment>
		<rdfs:comment xml:lang="OWLManchester">platform:implementsInterface some AndroidTestSuitebuilderAPI</rdfs:comment>
	</owl:Class>
	<owl:Class rdf:about="&android-1_6;AndroidTestSuitebuilderAnnotationClassLibrary">
		<owl:equivalentClass rdf:resource="&android-1_5;AndroidTestSuitebuilderAnnotationClassLibrary"/>
		<rdfs:subClassOf rdf:resource="&java;JavaClassLibrary"/>
		<rdfs:comment xml:lang="en">JavaLibrary implementing the android.test.suitebuilder.annotation package for Android 1.6</rdfs:comment>
		<rdfs:comment xml:lang="OWLManchester">platform:implementsInterface some AndroidTestSuitebuilderAnnotationAPI</rdfs:comment>
	</owl:Class>
	<owl:Class rdf:about="&android-1_6;JavaLangClassLibrary">
		<owl:equivalentClass rdf:resource="&android-1_5;JavaLangClassLibrary"/>
		<rdfs:subClassOf rdf:resource="&j2se-5_0;JavaLangClassLibrary"/>
		<rdfs:comment xml:lang="en">JavaLibrary implementing the java.lang package for Android 1.6</rdfs:comment>
		<rdfs:comment xml:lang="OWLManchester">platform:implementsInterface some JavaLangAPI</rdfs:comment>
	</owl:Class>
	<owl:Class rdf:about="&android-1_6;JavaLangAnnotationClassLibrary">
		<owl:equivalentClass rdf:resource="&j2se-5_0;JavaLangAnnotationClassLibrary"/>
		<owl:equivalentClass rdf:resource="&android-1_5;JavaLangAnnotationClassLibrary"/>
		<rdfs:subClassOf rdf:resource="&java;JavaClassLibrary"/>
		<rdfs:comment xml:lang="en">JavaLibrary implementing the java.lang.annotation package for Android 1.6</rdfs:comment>
		<rdfs:comment xml:lang="OWLManchester">platform:implementsInterface some JavaLangAnnotationAPI</rdfs:comment>
	</owl:Class>
	<owl:Class rdf:about="&android-1_6;JavaLangReflectClassLibrary">
		<owl:equivalentClass rdf:resource="&j2se-5_0;JavaLangReflectClassLibrary"/>
		<owl:equivalentClass rdf:resource="&android-1_5;JavaLangReflectClassLibrary"/>
		<rdfs:subClassOf rdf:resource="&java;JavaClassLibrary"/>
		<rdfs:comment xml:lang="en">JavaLibrary implementing the java.lang.reflect package for Android 1.6</rdfs:comment>
		<rdfs:comment xml:lang="OWLManchester">platform:implementsInterface some JavaLangReflectAPI</rdfs:comment>
	</owl:Class>
	<owl:Class rdf:about="&android-1_6;JavaLangRefClassLibrary">
		<owl:equivalentClass rdf:resource="&j2se-5_0;JavaLangRefClassLibrary"/>
		<owl:equivalentClass rdf:resource="&android-1_5;JavaLangRefClassLibrary"/>
		<rdfs:subClassOf rdf:resource="&java;JavaClassLibrary"/>
		<rdfs:comment xml:lang="en">JavaLibrary implementing the java.lang.ref package for Android 1.6</rdfs:comment>
		<rdfs:comment xml:lang="OWLManchester">platform:implementsInterface some JavaLangRefAPI</rdfs:comment>
	</owl:Class>
	<owl:Class rdf:about="&android-1_6;JavaUtilClassLibrary">
		<owl:equivalentClass rdf:resource="&j2se-5_0;JavaUtilClassLibrary"/>
		<owl:equivalentClass rdf:resource="&android-1_5;JavaUtilClassLibrary"/>
		<rdfs:subClassOf rdf:resource="&java;JavaClassLibrary"/>
		<rdfs:comment xml:lang="en">JavaLibrary implementing the java.util package for Android 1.6</rdfs:comment>
		<rdfs:comment xml:lang="OWLManchester">platform:implementsInterface some JavaUtilAPI</rdfs:comment>
	</owl:Class>
	<owl:Class rdf:about="&android-1_6;JavaUtilConcurrentClassLibrary">
		<owl:equivalentClass rdf:resource="&j2se-5_0;JavaUtilConcurrentClassLibrary"/>
		<owl:equivalentClass rdf:resource="&android-1_5;JavaUtilConcurrentClassLibrary"/>
		<rdfs:subClassOf rdf:resource="&java;JavaClassLibrary"/>
		<rdfs:comment xml:lang="en">JavaLibrary implementing the java.util.concurrent package for Android 1.6</rdfs:comment>
		<rdfs:comment xml:lang="OWLManchester">platform:implementsInterface some JavaUtilConcurrentAPI</rdfs:comment>
	</owl:Class>
	<owl:Class rdf:about="&android-1_6;JavaUtilConcurrentAtomicClassLibrary">
		<owl:equivalentClass rdf:resource="&j2se-5_0;JavaUtilConcurrentAtomicClassLibrary"/>
		<owl:equivalentClass rdf:resource="&android-1_5;JavaUtilConcurrentAtomicClassLibrary"/>
		<rdfs:subClassOf rdf:resource="&java;JavaClassLibrary"/>
		<rdfs:comment xml:lang="en">JavaLibrary implementing the java.util.concurrent.atomic package for Android 1.6</rdfs:comment>
		<rdfs:comment xml:lang="OWLManchester">platform:implementsInterface some JavaUtilConcurrentAtomicAPI</rdfs:comment>
	</owl:Class>
	<owl:Class rdf:about="&android-1_6;JavaUtilConcurrentLocksClassLibrary">
		<owl:equivalentClass rdf:resource="&j2se-5_0;JavaUtilConcurrentLocksClassLibrary"/>
		<owl:equivalentClass rdf:resource="&android-1_5;JavaUtilConcurrentLocksClassLibrary"/>
		<rdfs:subClassOf rdf:resource="&java;JavaClassLibrary"/>
		<rdfs:comment xml:lang="en">JavaLibrary implementing the java.util.concurrent.locks package for Android 1.6</rdfs:comment>
		<rdfs:comment xml:lang="OWLManchester">platform:implementsInterface some JavaUtilConcurrentLocksAPI</rdfs:comment>
	</owl:Class>
	<owl:Class rdf:about="&android-1_6;JavaUtilRegexClassLibrary">
		<owl:equivalentClass rdf:resource="&j2se-5_0;JavaUtilRegexClassLibrary"/>
		<owl:equivalentClass rdf:resource="&android-1_5;JavaUtilRegexClassLibrary"/>
		<rdfs:subClassOf rdf:resource="&java;JavaClassLibrary"/>
		<rdfs:comment xml:lang="en">JavaLibrary implementing the java.util.regex package for Android 1.6</rdfs:comment>
		<rdfs:comment xml:lang="OWLManchester">platform:implementsInterface some JavaUtilRegexAPI</rdfs:comment>
	</owl:Class>
	<owl:Class rdf:about="&android-1_6;JavaUtilJarClassLibrary">
		<owl:equivalentClass rdf:resource="&j2se-5_0;JavaUtilJarClassLibrary"/>
		<owl:equivalentClass rdf:resource="&android-1_5;JavaUtilJarClassLibrary"/>
		<rdfs:subClassOf rdf:resource="&java;JavaClassLibrary"/>
		<rdfs:comment xml:lang="en">JavaLibrary implementing the java.util.jar package for Android 1.6</rdfs:comment>
		<rdfs:comment xml:lang="OWLManchester">platform:implementsInterface some JavaUtilJarAPI</rdfs:comment>
	</owl:Class>
	<owl:Class rdf:about="&android-1_6;JavaUtilZipClassLibrary">
		<owl:equivalentClass rdf:resource="&j2se-5_0;JavaUtilZipClassLibrary"/>
		<owl:equivalentClass rdf:resource="&android-1_5;JavaUtilZipClassLibrary"/>
		<rdfs:subClassOf rdf:resource="&java;JavaClassLibrary"/>
		<rdfs:comment xml:lang="en">JavaLibrary implementing the java.util.zip package for Android 1.6</rdfs:comment>
		<rdfs:comment xml:lang="OWLManchester">platform:implementsInterface some JavaUtilZipAPI</rdfs:comment>
	</owl:Class>
	<owl:Class rdf:about="&android-1_6;JavaUtilLoggingClassLibrary">
		<owl:equivalentClass rdf:resource="&j2se-5_0;JavaUtilLoggingClassLibrary"/>
		<owl:equivalentClass rdf:resource="&android-1_5;JavaUtilLoggingClassLibrary"/>
		<rdfs:subClassOf rdf:resource="&java;JavaClassLibrary"/>
		<rdfs:comment xml:lang="en">JavaLibrary implementing the java.util.logging package for Android 1.6</rdfs:comment>
		<rdfs:comment xml:lang="OWLManchester">platform:implementsInterface some JavaUtilLoggingAPI</rdfs:comment>
	</owl:Class>
	<owl:Class rdf:about="&android-1_6;JavaUtilPrefsClassLibrary">
		<owl:equivalentClass rdf:resource="&j2se-5_0;JavaUtilPrefsClassLibrary"/>
		<owl:equivalentClass rdf:resource="&android-1_5;JavaUtilPrefsClassLibrary"/>
		<rdfs:subClassOf rdf:resource="&java;JavaClassLibrary"/>
		<rdfs:comment xml:lang="en">JavaLibrary implementing the java.util.prefs package for Android 1.6</rdfs:comment>
		<rdfs:comment xml:lang="OWLManchester">platform:implementsInterface some JavaUtilPrefsAPI</rdfs:comment>
	</owl:Class>
	<owl:Class rdf:about="&android-1_6;JavaIoClassLibrary">
		<owl:equivalentClass rdf:resource="&j2se-5_0;JavaIoClassLibrary"/>
		<owl:equivalentClass rdf:resource="&android-1_5;JavaIoClassLibrary"/>
		<rdfs:subClassOf rdf:resource="&java;JavaClassLibrary"/>
		<rdfs:comment xml:lang="en">JavaLibrary implementing the java.io package for Android 1.6</rdfs:comment>
		<rdfs:comment xml:lang="OWLManchester">platform:implementsInterface some JavaIoAPI</rdfs:comment>
	</owl:Class>
	<owl:Class rdf:about="&android-1_6;JavaNioClassLibrary">
		<owl:equivalentClass rdf:resource="&j2se-5_0;JavaNioClassLibrary"/>
		<owl:equivalentClass rdf:resource="&android-1_5;JavaNioClassLibrary"/>
		<rdfs:subClassOf rdf:resource="&java;JavaClassLibrary"/>
		<rdfs:comment xml:lang="en">JavaLibrary implementing the java.nio package for Android 1.6</rdfs:comment>
		<rdfs:comment xml:lang="OWLManchester">platform:implementsInterface some JavaNioAPI</rdfs:comment>
	</owl:Class>
	<owl:Class rdf:about="&android-1_6;JavaNioChannelsClassLibrary">
		<owl:equivalentClass rdf:resource="&j2se-5_0;JavaNioChannelsClassLibrary"/>
		<owl:equivalentClass rdf:resource="&android-1_5;JavaNioChannelsClassLibrary"/>
		<rdfs:subClassOf rdf:resource="&java;JavaClassLibrary"/>
		<rdfs:comment xml:lang="en">JavaLibrary implementing the java.nio.channels package for Android 1.6</rdfs:comment>
		<rdfs:comment xml:lang="OWLManchester">platform:implementsInterface some JavaNioChannelsAPI</rdfs:comment>
	</owl:Class>
	<owl:Class rdf:about="&android-1_6;JavaNioChannelsSpiClassLibrary">
		<owl:equivalentClass rdf:resource="&j2se-5_0;JavaNioChannelsSpiClassLibrary"/>
		<owl:equivalentClass rdf:resource="&android-1_5;JavaNioChannelsSpiClassLibrary"/>
		<rdfs:subClassOf rdf:resource="&java;JavaClassLibrary"/>
		<rdfs:comment xml:lang="en">JavaLibrary implementing the java.nio.channels.spi package for Android 1.6</rdfs:comment>
		<rdfs:comment xml:lang="OWLManchester">platform:implementsInterface some JavaNioChannelsSpiAPI</rdfs:comment>
	</owl:Class>
	<owl:Class rdf:about="&android-1_6;JavaNioCharsetClassLibrary">
		<owl:equivalentClass rdf:resource="&j2se-5_0;JavaNioCharsetClassLibrary"/>
		<owl:equivalentClass rdf:resource="&android-1_5;JavaNioCharsetClassLibrary"/>
		<rdfs:subClassOf rdf:resource="&java;JavaClassLibrary"/>
		<rdfs:comment xml:lang="en">JavaLibrary implementing the java.nio.charset package for Android 1.6</rdfs:comment>
		<rdfs:comment xml:lang="OWLManchester">platform:implementsInterface some JavaNioCharsetAPI</rdfs:comment>
	</owl:Class>
	<owl:Class rdf:about="&android-1_6;JavaNioCharsetSpiClassLibrary">
		<owl:equivalentClass rdf:resource="&j2se-5_0;JavaNioCharsetSpiClassLibrary"/>
		<owl:equivalentClass rdf:resource="&android-1_5;JavaNioCharsetSpiClassLibrary"/>
		<rdfs:subClassOf rdf:resource="&java;JavaClassLibrary"/>
		<rdfs:comment xml:lang="en">JavaLibrary implementing the java.nio.charset.spi package for Android 1.6</rdfs:comment>
		<rdfs:comment xml:lang="OWLManchester">platform:implementsInterface some JavaNioCharsetSpiAPI</rdfs:comment>
	</owl:Class>
	<owl:Class rdf:about="&android-1_6;JavaNetClassLibrary">
		<owl:equivalentClass rdf:resource="&j2se-5_0;JavaNetClassLibrary"/>
		<owl:equivalentClass rdf:resource="&android-1_5;JavaNetClassLibrary"/>
		<rdfs:subClassOf rdf:resource="&java;JavaClassLibrary"/>
		<rdfs:comment xml:lang="en">JavaLibrary implementing the java.net package for Android 1.6</rdfs:comment>
		<rdfs:comment xml:lang="OWLManchester">platform:implementsInterface some JavaNetAPI</rdfs:comment>
	</owl:Class>
	<owl:Class rdf:about="&android-1_6;JavaSecurityClassLibrary">
		<owl:equivalentClass rdf:resource="&j2se-5_0;JavaSecurityClassLibrary"/>
		<owl:equivalentClass rdf:resource="&android-1_5;JavaSecurityClassLibrary"/>
		<rdfs:subClassOf rdf:resource="&java;JavaClassLibrary"/>
		<rdfs:comment xml:lang="en">JavaLibrary implementing the java.security package for Android 1.6</rdfs:comment>
		<rdfs:comment xml:lang="OWLManchester">platform:implementsInterface some JavaSecurityAPI</rdfs:comment>
	</owl:Class>
	<owl:Class rdf:about="&android-1_6;JavaSecurityCertClassLibrary">
		<owl:equivalentClass rdf:resource="&j2se-5_0;JavaSecurityCertClassLibrary"/>
		<owl:equivalentClass rdf:resource="&android-1_5;JavaSecurityCertClassLibrary"/>
		<rdfs:subClassOf rdf:resource="&java;JavaClassLibrary"/>
		<rdfs:comment xml:lang="en">JavaLibrary implementing the java.security.cert package for Android 1.6</rdfs:comment>
		<rdfs:comment xml:lang="OWLManchester">platform:implementsInterface some JavaSecurityCertAPI</rdfs:comment>
	</owl:Class>
	<owl:Class rdf:about="&android-1_6;JavaSecuritySpecClassLibrary">
		<owl:equivalentClass rdf:resource="&j2se-5_0;JavaSecuritySpecClassLibrary"/>
		<owl:equivalentClass rdf:resource="&android-1_5;JavaSecuritySpecClassLibrary"/>
		<rdfs:subClassOf rdf:resource="&java;JavaClassLibrary"/>
		<rdfs:comment xml:lang="en">JavaLibrary implementing the java.security.spec package for Android 1.6</rdfs:comment>
		<rdfs:comment xml:lang="OWLManchester">platform:implementsInterface some JavaSecuritySpecAPI</rdfs:comment>
	</owl:Class>
	<owl:Class rdf:about="&android-1_6;JavaSecurityAclClassLibrary">
		<owl:equivalentClass rdf:resource="&j2se-5_0;JavaSecurityAclClassLibrary"/>
		<owl:equivalentClass rdf:resource="&android-1_5;JavaSecurityAclClassLibrary"/>
		<rdfs:subClassOf rdf:resource="&java;JavaClassLibrary"/>
		<rdfs:comment xml:lang="en">JavaLibrary implementing the java.security.acl package for Android 1.6</rdfs:comment>
		<rdfs:comment xml:lang="OWLManchester">platform:implementsInterface some JavaSecurityAclAPI</rdfs:comment>
	</owl:Class>
	<owl:Class rdf:about="&android-1_6;JavaSecurityInterfacesClassLibrary">
		<owl:equivalentClass rdf:resource="&j2se-5_0;JavaSecurityInterfacesClassLibrary"/>
		<owl:equivalentClass rdf:resource="&android-1_5;JavaSecurityInterfacesClassLibrary"/>
		<rdfs:subClassOf rdf:resource="&java;JavaClassLibrary"/>
		<rdfs:comment xml:lang="en">JavaLibrary implementing the java.security.interfaces package for Android 1.6</rdfs:comment>
		<rdfs:comment xml:lang="OWLManchester">platform:implementsInterface some JavaSecurityInterfacesAPI</rdfs:comment>
	</owl:Class>
	<owl:Class rdf:about="&android-1_6;JavaTextClassLibrary">
		<owl:equivalentClass rdf:resource="&j2se-5_0;JavaTextClassLibrary"/>
		<owl:equivalentClass rdf:resource="&android-1_5;JavaTextClassLibrary"/>
		<rdfs:subClassOf rdf:resource="&java;JavaClassLibrary"/>
		<rdfs:comment xml:lang="en">JavaLibrary implementing the java.text package for Android 1.6</rdfs:comment>
		<rdfs:comment xml:lang="OWLManchester">platform:implementsInterface some JavaTextAPI</rdfs:comment>
	</owl:Class>
	<owl:Class rdf:about="&android-1_6;JavaAwtFontClassLibrary">
		<owl:equivalentClass rdf:resource="&android-1_5;JavaAwtFontClassLibrary"/>
		<rdfs:subClassOf rdf:resource="&java;JavaClassLibrary"/>
		<rdfs:comment xml:lang="en">JavaLibrary implementing the java.awt.font package for Android 1.6</rdfs:comment>
		<rdfs:comment xml:lang="OWLManchester">platform:implementsInterface some JavaAwtFontAPI</rdfs:comment>
	</owl:Class>
	<owl:Class rdf:about="&android-1_6;JavaBeansClassLibrary">
		<owl:equivalentClass rdf:resource="&android-1_5;JavaBeansClassLibrary"/>
		<rdfs:subClassOf rdf:resource="&java;JavaClassLibrary"/>
		<rdfs:comment xml:lang="en">JavaLibrary implementing the java.beans package for Android 1.6</rdfs:comment>
		<rdfs:comment xml:lang="OWLManchester">platform:implementsInterface some JavaBeansAPI</rdfs:comment>
	</owl:Class>
	<owl:Class rdf:about="&android-1_6;JavaMathClassLibrary">
		<owl:equivalentClass rdf:resource="&j2se-5_0;JavaMathClassLibrary"/>
		<owl:equivalentClass rdf:resource="&android-1_5;JavaMathClassLibrary"/>
		<rdfs:subClassOf rdf:resource="&java;JavaClassLibrary"/>
		<rdfs:comment xml:lang="en">JavaLibrary implementing the java.math package for Android 1.6</rdfs:comment>
		<rdfs:comment xml:lang="OWLManchester">platform:implementsInterface some JavaMathAPI</rdfs:comment>
	</owl:Class>
	<owl:Class rdf:about="&android-1_6;JavaSqlClassLibrary">
		<owl:equivalentClass rdf:resource="&j2se-5_0;JavaSqlClassLibrary"/>
		<owl:equivalentClass rdf:resource="&android-1_5;JavaSqlClassLibrary"/>
		<rdfs:subClassOf rdf:resource="&java;JavaClassLibrary"/>
		<rdfs:comment xml:lang="en">JavaLibrary implementing the java.sql package for Android 1.6</rdfs:comment>
		<rdfs:comment xml:lang="OWLManchester">platform:implementsInterface some JavaSqlAPI</rdfs:comment>
	</owl:Class>
	<owl:Class rdf:about="&android-1_6;OrgXmlpullV1ClassLibrary">
		<owl:equivalentClass rdf:resource="&android-1_5;OrgXmlpullV1ClassLibrary"/>
		<rdfs:subClassOf rdf:resource="&java;JavaClassLibrary"/>
		<rdfs:comment xml:lang="en">JavaLibrary implementing the org.xmlpull.v1 package for Android 1.6</rdfs:comment>
		<rdfs:comment xml:lang="OWLManchester">platform:implementsInterface some OrgXmlpullV1API</rdfs:comment>
	</owl:Class>
	<owl:Class rdf:about="&android-1_6;OrgXmlpullV1Sax2ClassLibrary">
		<owl:equivalentClass rdf:resource="&android-1_5;OrgXmlpullV1Sax2ClassLibrary"/>
		<rdfs:subClassOf rdf:resource="&java;JavaClassLibrary"/>
		<rdfs:comment xml:lang="en">JavaLibrary implementing the org.xmlpull.v1.sax2 package for Android 1.6</rdfs:comment>
		<rdfs:comment xml:lang="OWLManchester">platform:implementsInterface some OrgXmlpullV1Sax2API</rdfs:comment>
	</owl:Class>
	<owl:Class rdf:about="&android-1_6;OrgXmlSaxClassLibrary">
		<owl:equivalentClass rdf:resource="&j2se-5_0;OrgXmlSaxClassLibrary"/>
		<owl:equivalentClass rdf:resource="&android-1_5;OrgXmlSaxClassLibrary"/>
		<rdfs:subClassOf rdf:resource="&java;JavaClassLibrary"/>
		<rdfs:comment xml:lang="en">JavaLibrary implementing the org.xml.sax package for Android 1.6</rdfs:comment>
		<rdfs:comment xml:lang="OWLManchester">platform:implementsInterface some OrgXmlSaxAPI</rdfs:comment>
	</owl:Class>
	<owl:Class rdf:about="&android-1_6;OrgXmlSaxHelpersClassLibrary">
		<owl:equivalentClass rdf:resource="&j2se-5_0;OrgXmlSaxHelpersClassLibrary"/>
		<owl:equivalentClass rdf:resource="&android-1_5;OrgXmlSaxHelpersClassLibrary"/>
		<rdfs:subClassOf rdf:resource="&java;JavaClassLibrary"/>
		<rdfs:comment xml:lang="en">JavaLibrary implementing the org.xml.sax.helpers package for Android 1.6</rdfs:comment>
		<rdfs:comment xml:lang="OWLManchester">platform:implementsInterface some OrgXmlSaxHelpersAPI</rdfs:comment>
	</owl:Class>
	<owl:Class rdf:about="&android-1_6;OrgXmlSaxExtClassLibrary">
		<owl:equivalentClass rdf:resource="&j2se-5_0;OrgXmlSaxExtClassLibrary"/>
		<owl:equivalentClass rdf:resource="&android-1_5;OrgXmlSaxExtClassLibrary"/>
		<rdfs:subClassOf rdf:resource="&java;JavaClassLibrary"/>
		<rdfs:comment xml:lang="en">JavaLibrary implementing the org.xml.sax.ext package for Android 1.6</rdfs:comment>
		<rdfs:comment xml:lang="OWLManchester">platform:implementsInterface some OrgXmlSaxExtAPI</rdfs:comment>
	</owl:Class>
	<owl:Class rdf:about="&android-1_6;OrgW3cDomClassLibrary">
		<owl:equivalentClass rdf:resource="&android-1_5;OrgW3cDomClassLibrary"/>
		<rdfs:subClassOf rdf:resource="&java;JavaClassLibrary"/>
		<rdfs:comment xml:lang="en">JavaLibrary implementing the org.w3c.dom package for Android 1.6</rdfs:comment>
		<rdfs:comment xml:lang="OWLManchester">platform:implementsInterface some OrgW3cDomAPI</rdfs:comment>
	</owl:Class>
	<owl:Class rdf:about="&android-1_6;OrgApacheCommonsLoggingClassLibrary">
		<owl:equivalentClass rdf:resource="&android-1_5;OrgApacheCommonsLoggingClassLibrary"/>
		<rdfs:subClassOf rdf:resource="&java;JavaClassLibrary"/>
		<rdfs:comment xml:lang="en">JavaLibrary implementing the org.apache.commons.logging package for Android 1.6</rdfs:comment>
		<rdfs:comment xml:lang="OWLManchester">platform:implementsInterface some OrgApacheCommonsLoggingAPI</rdfs:comment>
	</owl:Class>
	<owl:Class rdf:about="&android-1_6;OrgApacheHttpClassLibrary">
		<owl:equivalentClass rdf:resource="&android-1_5;OrgApacheHttpClassLibrary"/>
		<rdfs:subClassOf rdf:resource="&java;JavaClassLibrary"/>
		<rdfs:comment xml:lang="en">JavaLibrary implementing the org.apache.http package for Android 1.6</rdfs:comment>
		<rdfs:comment xml:lang="OWLManchester">platform:implementsInterface some OrgApacheHttpAPI</rdfs:comment>
	</owl:Class>
	<owl:Class rdf:about="&android-1_6;OrgApacheHttpProtocolClassLibrary">
		<owl:equivalentClass rdf:resource="&android-1_5;OrgApacheHttpProtocolClassLibrary"/>
		<rdfs:subClassOf rdf:resource="&java;JavaClassLibrary"/>
		<rdfs:comment xml:lang="en">JavaLibrary implementing the org.apache.http.protocol package for Android 1.6</rdfs:comment>
		<rdfs:comment xml:lang="OWLManchester">platform:implementsInterface some OrgApacheHttpProtocolAPI</rdfs:comment>
	</owl:Class>
	<owl:Class rdf:about="&android-1_6;OrgApacheHttpUtilClassLibrary">
		<owl:equivalentClass rdf:resource="&android-1_5;OrgApacheHttpUtilClassLibrary"/>
		<rdfs:subClassOf rdf:resource="&java;JavaClassLibrary"/>
		<rdfs:comment xml:lang="en">JavaLibrary implementing the org.apache.http.util package for Android 1.6</rdfs:comment>
		<rdfs:comment xml:lang="OWLManchester">platform:implementsInterface some OrgApacheHttpUtilAPI</rdfs:comment>
	</owl:Class>
	<owl:Class rdf:about="&android-1_6;OrgApacheHttpParamsClassLibrary">
		<owl:equivalentClass rdf:resource="&android-1_5;OrgApacheHttpParamsClassLibrary"/>
		<rdfs:subClassOf rdf:resource="&java;JavaClassLibrary"/>
		<rdfs:comment xml:lang="en">JavaLibrary implementing the org.apache.http.params package for Android 1.6</rdfs:comment>
		<rdfs:comment xml:lang="OWLManchester">platform:implementsInterface some OrgApacheHttpParamsAPI</rdfs:comment>
	</owl:Class>
	<owl:Class rdf:about="&android-1_6;OrgApacheHttpAuthClassLibrary">
		<owl:equivalentClass rdf:resource="&android-1_5;OrgApacheHttpAuthClassLibrary"/>
		<rdfs:subClassOf rdf:resource="&java;JavaClassLibrary"/>
		<rdfs:comment xml:lang="en">JavaLibrary implementing the org.apache.http.auth package for Android 1.6</rdfs:comment>
		<rdfs:comment xml:lang="OWLManchester">platform:implementsInterface some OrgApacheHttpAuthAPI</rdfs:comment>
	</owl:Class>
	<owl:Class rdf:about="&android-1_6;OrgApacheHttpAuthParamsClassLibrary">
		<owl:equivalentClass rdf:resource="&android-1_5;OrgApacheHttpAuthParamsClassLibrary"/>
		<rdfs:subClassOf rdf:resource="&java;JavaClassLibrary"/>
		<rdfs:comment xml:lang="en">JavaLibrary implementing the org.apache.http.auth.params package for Android 1.6</rdfs:comment>
		<rdfs:comment xml:lang="OWLManchester">platform:implementsInterface some OrgApacheHttpAuthParamsAPI</rdfs:comment>
	</owl:Class>
	<owl:Class rdf:about="&android-1_6;OrgApacheHttpClientClassLibrary">
		<owl:equivalentClass rdf:resource="&android-1_5;OrgApacheHttpClientClassLibrary"/>
		<rdfs:subClassOf rdf:resource="&java;JavaClassLibrary"/>
		<rdfs:comment xml:lang="en">JavaLibrary implementing the org.apache.http.client package for Android 1.6</rdfs:comment>
		<rdfs:comment xml:lang="OWLManchester">platform:implementsInterface some OrgApacheHttpClientAPI</rdfs:comment>
	</owl:Class>
	<owl:Class rdf:about="&android-1_6;OrgApacheHttpClientMethodsClassLibrary">
		<owl:equivalentClass rdf:resource="&android-1_5;OrgApacheHttpClientMethodsClassLibrary"/>
		<rdfs:subClassOf rdf:resource="&java;JavaClassLibrary"/>
		<rdfs:comment xml:lang="en">JavaLibrary implementing the org.apache.http.client.methods package for Android 1.6</rdfs:comment>
		<rdfs:comment xml:lang="OWLManchester">platform:implementsInterface some OrgApacheHttpClientMethodsAPI</rdfs:comment>
	</owl:Class>
	<owl:Class rdf:about="&android-1_6;OrgApacheHttpClientEntityClassLibrary">
		<owl:equivalentClass rdf:resource="&android-1_5;OrgApacheHttpClientEntityClassLibrary"/>
		<rdfs:subClassOf rdf:resource="&java;JavaClassLibrary"/>
		<rdfs:comment xml:lang="en">JavaLibrary implementing the org.apache.http.client.entity package for Android 1.6</rdfs:comment>
		<rdfs:comment xml:lang="OWLManchester">platform:implementsInterface some OrgApacheHttpClientEntityAPI</rdfs:comment>
	</owl:Class>
	<owl:Class rdf:about="&android-1_6;OrgApacheHttpClientParamsClassLibrary">
		<owl:equivalentClass rdf:resource="&android-1_5;OrgApacheHttpClientParamsClassLibrary"/>
		<rdfs:subClassOf rdf:resource="&java;JavaClassLibrary"/>
		<rdfs:comment xml:lang="en">JavaLibrary implementing the org.apache.http.client.params package for Android 1.6</rdfs:comment>
		<rdfs:comment xml:lang="OWLManchester">platform:implementsInterface some OrgApacheHttpClientParamsAPI</rdfs:comment>
	</owl:Class>
	<owl:Class rdf:about="&android-1_6;OrgApacheHttpClientProtocolClassLibrary">
		<owl:equivalentClass rdf:resource="&android-1_5;OrgApacheHttpClientProtocolClassLibrary"/>
		<rdfs:subClassOf rdf:resource="&java;JavaClassLibrary"/>
		<rdfs:comment xml:lang="en">JavaLibrary implementing the org.apache.http.client.protocol package for Android 1.6</rdfs:comment>
		<rdfs:comment xml:lang="OWLManchester">platform:implementsInterface some OrgApacheHttpClientProtocolAPI</rdfs:comment>
	</owl:Class>
	<owl:Class rdf:about="&android-1_6;OrgApacheHttpClientUtilsClassLibrary">
		<owl:equivalentClass rdf:resource="&android-1_5;OrgApacheHttpClientUtilsClassLibrary"/>
		<rdfs:subClassOf rdf:resource="&java;JavaClassLibrary"/>
		<rdfs:comment xml:lang="en">JavaLibrary implementing the org.apache.http.client.utils package for Android 1.6</rdfs:comment>
		<rdfs:comment xml:lang="OWLManchester">platform:implementsInterface some OrgApacheHttpClientUtilsAPI</rdfs:comment>
	</owl:Class>
	<owl:Class rdf:about="&android-1_6;OrgApacheHttpCookieClassLibrary">
		<owl:equivalentClass rdf:resource="&android-1_5;OrgApacheHttpCookieClassLibrary"/>
		<rdfs:subClassOf rdf:resource="&java;JavaClassLibrary"/>
		<rdfs:comment xml:lang="en">JavaLibrary implementing the org.apache.http.cookie package for Android 1.6</rdfs:comment>
		<rdfs:comment xml:lang="OWLManchester">platform:implementsInterface some OrgApacheHttpCookieAPI</rdfs:comment>
	</owl:Class>
	<owl:Class rdf:about="&android-1_6;OrgApacheHttpCookieParamsClassLibrary">
		<owl:equivalentClass rdf:resource="&android-1_5;OrgApacheHttpCookieParamsClassLibrary"/>
		<rdfs:subClassOf rdf:resource="&java;JavaClassLibrary"/>
		<rdfs:comment xml:lang="en">JavaLibrary implementing the org.apache.http.cookie.params package for Android 1.6</rdfs:comment>
		<rdfs:comment xml:lang="OWLManchester">platform:implementsInterface some OrgApacheHttpCookieParamsAPI</rdfs:comment>
	</owl:Class>
	<owl:Class rdf:about="&android-1_6;OrgApacheHttpConnClassLibrary">
		<owl:equivalentClass rdf:resource="&android-1_5;OrgApacheHttpConnClassLibrary"/>
		<rdfs:subClassOf rdf:resource="&java;JavaClassLibrary"/>
		<rdfs:comment xml:lang="en">JavaLibrary implementing the org.apache.http.conn package for Android 1.6</rdfs:comment>
		<rdfs:comment xml:lang="OWLManchester">platform:implementsInterface some OrgApacheHttpConnAPI</rdfs:comment>
	</owl:Class>
	<owl:Class rdf:about="&android-1_6;OrgApacheHttpConnParamsClassLibrary">
		<owl:equivalentClass rdf:resource="&android-1_5;OrgApacheHttpConnParamsClassLibrary"/>
		<rdfs:subClassOf rdf:resource="&java;JavaClassLibrary"/>
		<rdfs:comment xml:lang="en">JavaLibrary implementing the org.apache.http.conn.params package for Android 1.6</rdfs:comment>
		<rdfs:comment xml:lang="OWLManchester">platform:implementsInterface some OrgApacheHttpConnParamsAPI</rdfs:comment>
	</owl:Class>
	<owl:Class rdf:about="&android-1_6;OrgApacheHttpConnSchemeClassLibrary">
		<owl:equivalentClass rdf:resource="&android-1_5;OrgApacheHttpConnSchemeClassLibrary"/>
		<rdfs:subClassOf rdf:resource="&java;JavaClassLibrary"/>
		<rdfs:comment xml:lang="en">JavaLibrary implementing the org.apache.http.conn.scheme package for Android 1.6</rdfs:comment>
		<rdfs:comment xml:lang="OWLManchester">platform:implementsInterface some OrgApacheHttpConnSchemeAPI</rdfs:comment>
	</owl:Class>
	<owl:Class rdf:about="&android-1_6;OrgApacheHttpConnRoutingClassLibrary">
		<owl:equivalentClass rdf:resource="&android-1_5;OrgApacheHttpConnRoutingClassLibrary"/>
		<rdfs:subClassOf rdf:resource="&java;JavaClassLibrary"/>
		<rdfs:comment xml:lang="en">JavaLibrary implementing the org.apache.http.conn.routing package for Android 1.6</rdfs:comment>
		<rdfs:comment xml:lang="OWLManchester">platform:implementsInterface some OrgApacheHttpConnRoutingAPI</rdfs:comment>
	</owl:Class>
	<owl:Class rdf:about="&android-1_6;OrgApacheHttpConnSslClassLibrary">
		<owl:equivalentClass rdf:resource="&android-1_5;OrgApacheHttpConnSslClassLibrary"/>
		<rdfs:subClassOf rdf:resource="&java;JavaClassLibrary"/>
		<rdfs:comment xml:lang="en">JavaLibrary implementing the org.apache.http.conn.ssl package for Android 1.6</rdfs:comment>
		<rdfs:comment xml:lang="OWLManchester">platform:implementsInterface some OrgApacheHttpConnSslAPI</rdfs:comment>
	</owl:Class>
	<owl:Class rdf:about="&android-1_6;OrgApacheHttpConnUtilClassLibrary">
		<owl:equivalentClass rdf:resource="&android-1_5;OrgApacheHttpConnUtilClassLibrary"/>
		<rdfs:subClassOf rdf:resource="&java;JavaClassLibrary"/>
		<rdfs:comment xml:lang="en">JavaLibrary implementing the org.apache.http.conn.util package for Android 1.6</rdfs:comment>
		<rdfs:comment xml:lang="OWLManchester">platform:implementsInterface some OrgApacheHttpConnUtilAPI</rdfs:comment>
	</owl:Class>
	<owl:Class rdf:about="&android-1_6;OrgApacheHttpEntityClassLibrary">
		<owl:equivalentClass rdf:resource="&android-1_5;OrgApacheHttpEntityClassLibrary"/>
		<rdfs:subClassOf rdf:resource="&java;JavaClassLibrary"/>
		<rdfs:comment xml:lang="en">JavaLibrary implementing the org.apache.http.entity package for Android 1.6</rdfs:comment>
		<rdfs:comment xml:lang="OWLManchester">platform:implementsInterface some OrgApacheHttpEntityAPI</rdfs:comment>
	</owl:Class>
	<owl:Class rdf:about="&android-1_6;OrgApacheHttpMessageClassLibrary">
		<owl:equivalentClass rdf:resource="&android-1_5;OrgApacheHttpMessageClassLibrary"/>
		<rdfs:subClassOf rdf:resource="&java;JavaClassLibrary"/>
		<rdfs:comment xml:lang="en">JavaLibrary implementing the org.apache.http.message package for Android 1.6</rdfs:comment>
		<rdfs:comment xml:lang="OWLManchester">platform:implementsInterface some OrgApacheHttpMessageAPI</rdfs:comment>
	</owl:Class>
	<owl:Class rdf:about="&android-1_6;OrgApacheHttpImplClassLibrary">
		<owl:equivalentClass rdf:resource="&android-1_5;OrgApacheHttpImplClassLibrary"/>
		<rdfs:subClassOf rdf:resource="&java;JavaClassLibrary"/>
		<rdfs:comment xml:lang="en">JavaLibrary implementing the org.apache.http.impl package for Android 1.6</rdfs:comment>
		<rdfs:comment xml:lang="OWLManchester">platform:implementsInterface some OrgApacheHttpImplAPI</rdfs:comment>
	</owl:Class>
	<owl:Class rdf:about="&android-1_6;OrgApacheHttpImplEntityClassLibrary">
		<owl:equivalentClass rdf:resource="&android-1_5;OrgApacheHttpImplEntityClassLibrary"/>
		<rdfs:subClassOf rdf:resource="&java;JavaClassLibrary"/>
		<rdfs:comment xml:lang="en">JavaLibrary implementing the org.apache.http.impl.entity package for Android 1.6</rdfs:comment>
		<rdfs:comment xml:lang="OWLManchester">platform:implementsInterface some OrgApacheHttpImplEntityAPI</rdfs:comment>
	</owl:Class>
	<owl:Class rdf:about="&android-1_6;OrgApacheHttpImplAuthClassLibrary">
		<owl:equivalentClass rdf:resource="&android-1_5;OrgApacheHttpImplAuthClassLibrary"/>
		<rdfs:subClassOf rdf:resource="&java;JavaClassLibrary"/>
		<rdfs:comment xml:lang="en">JavaLibrary implementing the org.apache.http.impl.auth package for Android 1.6</rdfs:comment>
		<rdfs:comment xml:lang="OWLManchester">platform:implementsInterface some OrgApacheHttpImplAuthAPI</rdfs:comment>
	</owl:Class>
	<owl:Class rdf:about="&android-1_6;OrgApacheHttpImplClientClassLibrary">
		<owl:equivalentClass rdf:resource="&android-1_5;OrgApacheHttpImplClientClassLibrary"/>
		<rdfs:subClassOf rdf:resource="&java;JavaClassLibrary"/>
		<rdfs:comment xml:lang="en">JavaLibrary implementing the org.apache.http.impl.client package for Android 1.6</rdfs:comment>
		<rdfs:comment xml:lang="OWLManchester">platform:implementsInterface some OrgApacheHttpImplClientAPI</rdfs:comment>
	</owl:Class>
	<owl:Class rdf:about="&android-1_6;OrgApacheHttpImplConnClassLibrary">
		<owl:equivalentClass rdf:resource="&android-1_5;OrgApacheHttpImplConnClassLibrary"/>
		<rdfs:subClassOf rdf:resource="&java;JavaClassLibrary"/>
		<rdfs:comment xml:lang="en">JavaLibrary implementing the org.apache.http.impl.conn package for Android 1.6</rdfs:comment>
		<rdfs:comment xml:lang="OWLManchester">platform:implementsInterface some OrgApacheHttpImplConnAPI</rdfs:comment>
	</owl:Class>
	<owl:Class rdf:about="&android-1_6;OrgApacheHttpImplConnTsccmClassLibrary">
		<owl:equivalentClass rdf:resource="&android-1_5;OrgApacheHttpImplConnTsccmClassLibrary"/>
		<rdfs:subClassOf rdf:resource="&java;JavaClassLibrary"/>
		<rdfs:comment xml:lang="en">JavaLibrary implementing the org.apache.http.impl.conn.tsccm package for Android 1.6</rdfs:comment>
		<rdfs:comment xml:lang="OWLManchester">platform:implementsInterface some OrgApacheHttpImplConnTsccmAPI</rdfs:comment>
	</owl:Class>
	<owl:Class rdf:about="&android-1_6;OrgApacheHttpImplIoClassLibrary">
		<owl:equivalentClass rdf:resource="&android-1_5;OrgApacheHttpImplIoClassLibrary"/>
		<rdfs:subClassOf rdf:resource="&java;JavaClassLibrary"/>
		<rdfs:comment xml:lang="en">JavaLibrary implementing the org.apache.http.impl.io package for Android 1.6</rdfs:comment>
		<rdfs:comment xml:lang="OWLManchester">platform:implementsInterface some OrgApacheHttpImplIoAPI</rdfs:comment>
	</owl:Class>
	<owl:Class rdf:about="&android-1_6;OrgApacheHttpImplCookieClassLibrary">
		<owl:equivalentClass rdf:resource="&android-1_5;OrgApacheHttpImplCookieClassLibrary"/>
		<rdfs:subClassOf rdf:resource="&java;JavaClassLibrary"/>
		<rdfs:comment xml:lang="en">JavaLibrary implementing the org.apache.http.impl.cookie package for Android 1.6</rdfs:comment>
		<rdfs:comment xml:lang="OWLManchester">platform:implementsInterface some OrgApacheHttpImplCookieAPI</rdfs:comment>
	</owl:Class>
	<owl:Class rdf:about="&android-1_6;OrgApacheHttpIoClassLibrary">
		<owl:equivalentClass rdf:resource="&android-1_5;OrgApacheHttpIoClassLibrary"/>
		<rdfs:subClassOf rdf:resource="&java;JavaClassLibrary"/>
		<rdfs:comment xml:lang="en">JavaLibrary implementing the org.apache.http.io package for Android 1.6</rdfs:comment>
		<rdfs:comment xml:lang="OWLManchester">platform:implementsInterface some OrgApacheHttpIoAPI</rdfs:comment>
	</owl:Class>
	<owl:Class rdf:about="&android-1_6;OrgJsonClassLibrary">
		<owl:equivalentClass rdf:resource="&android-1_5;OrgJsonClassLibrary"/>
		<rdfs:subClassOf rdf:resource="&java;JavaClassLibrary"/>
		<rdfs:comment xml:lang="en">JavaLibrary implementing the org.json package for Android 1.6</rdfs:comment>
		<rdfs:comment xml:lang="OWLManchester">platform:implementsInterface some OrgJsonAPI</rdfs:comment>
	</owl:Class>
	<owl:Class rdf:about="&android-1_6;JavaxMicroeditionKhronosOpenglesClassLibrary">
		<owl:equivalentClass rdf:resource="&android-1_5;JavaxMicroeditionKhronosOpenglesClassLibrary"/>
		<rdfs:subClassOf rdf:resource="&java;JavaClassLibrary"/>
		<rdfs:comment xml:lang="en">JavaLibrary implementing the javax.microedition.khronos.opengles package for Android 1.6</rdfs:comment>
		<rdfs:comment xml:lang="OWLManchester">platform:implementsInterface some JavaxMicroeditionKhronosOpenglesAPI</rdfs:comment>
	</owl:Class>
	<owl:Class rdf:about="&android-1_6;JavaxMicroeditionKhronosEglClassLibrary">
		<owl:equivalentClass rdf:resource="&android-1_5;JavaxMicroeditionKhronosEglClassLibrary"/>
		<rdfs:subClassOf rdf:resource="&java;JavaClassLibrary"/>
		<rdfs:comment xml:lang="en">JavaLibrary implementing the javax.microedition.khronos.egl package for Android 1.6</rdfs:comment>
		<rdfs:comment xml:lang="OWLManchester">platform:implementsInterface some JavaxMicroeditionKhronosEglAPI</rdfs:comment>
	</owl:Class>
	<owl:Class rdf:about="&android-1_6;JavaxNetClassLibrary">
		<owl:equivalentClass rdf:resource="&j2se-5_0;JavaxNetClassLibrary"/>
		<owl:equivalentClass rdf:resource="&android-1_5;JavaxNetClassLibrary"/>
		<rdfs:subClassOf rdf:resource="&java;JavaClassLibrary"/>
		<rdfs:comment xml:lang="en">JavaLibrary implementing the javax.net package for Android 1.6</rdfs:comment>
		<rdfs:comment xml:lang="OWLManchester">platform:implementsInterface some JavaxNetAPI</rdfs:comment>
	</owl:Class>
	<owl:Class rdf:about="&android-1_6;JavaxNetSslClassLibrary">
		<owl:equivalentClass rdf:resource="&j2se-5_0;JavaxNetSslClassLibrary"/>
		<owl:equivalentClass rdf:resource="&android-1_5;JavaxNetSslClassLibrary"/>
		<rdfs:subClassOf rdf:resource="&java;JavaClassLibrary"/>
		<rdfs:comment xml:lang="en">JavaLibrary implementing the javax.net.ssl package for Android 1.6</rdfs:comment>
		<rdfs:comment xml:lang="OWLManchester">platform:implementsInterface some JavaxNetSslAPI</rdfs:comment>
	</owl:Class>
	<owl:Class rdf:about="&android-1_6;JavaxSecurityAuthClassLibrary">
		<owl:equivalentClass rdf:resource="&android-1_5;JavaxSecurityAuthClassLibrary"/>
		<rdfs:subClassOf rdf:resource="&java;JavaClassLibrary"/>
		<rdfs:comment xml:lang="en">JavaLibrary implementing the javax.security.auth package for Android 1.6</rdfs:comment>
		<rdfs:comment xml:lang="OWLManchester">platform:implementsInterface some JavaxSecurityAuthAPI</rdfs:comment>
	</owl:Class>
	<owl:Class rdf:about="&android-1_6;JavaxSecurityAuthCallbackClassLibrary">
		<owl:equivalentClass rdf:resource="&android-1_5;JavaxSecurityAuthCallbackClassLibrary"/>
		<rdfs:subClassOf rdf:resource="&java;JavaClassLibrary"/>
		<rdfs:comment xml:lang="en">JavaLibrary implementing the javax.security.auth.callback package for Android 1.6</rdfs:comment>
		<rdfs:comment xml:lang="OWLManchester">platform:implementsInterface some JavaxSecurityAuthCallbackAPI</rdfs:comment>
	</owl:Class>
	<owl:Class rdf:about="&android-1_6;JavaxSecurityAuthX500ClassLibrary">
		<owl:equivalentClass rdf:resource="&android-1_5;JavaxSecurityAuthX500ClassLibrary"/>
		<rdfs:subClassOf rdf:resource="&java;JavaClassLibrary"/>
		<rdfs:comment xml:lang="en">JavaLibrary implementing the javax.security.auth.x500 package for Android 1.6</rdfs:comment>
		<rdfs:comment xml:lang="OWLManchester">platform:implementsInterface some JavaxSecurityAuthX500API</rdfs:comment>
	</owl:Class>
	<owl:Class rdf:about="&android-1_6;JavaxSecurityAuthLoginClassLibrary">
		<owl:equivalentClass rdf:resource="&android-1_5;JavaxSecurityAuthLoginClassLibrary"/>
		<rdfs:subClassOf rdf:resource="&java;JavaClassLibrary"/>
		<rdfs:comment xml:lang="en">JavaLibrary implementing the javax.security.auth.login package for Android 1.6</rdfs:comment>
		<rdfs:comment xml:lang="OWLManchester">platform:implementsInterface some JavaxSecurityAuthLoginAPI</rdfs:comment>
	</owl:Class>
	<owl:Class rdf:about="&android-1_6;JavaxSecurityCertClassLibrary">
		<owl:equivalentClass rdf:resource="&j2se-5_0;JavaxSecurityCertClassLibrary"/>
		<owl:equivalentClass rdf:resource="&android-1_5;JavaxSecurityCertClassLibrary"/>
		<rdfs:subClassOf rdf:resource="&java;JavaClassLibrary"/>
		<rdfs:comment xml:lang="en">JavaLibrary implementing the javax.security.cert package for Android 1.6</rdfs:comment>
		<rdfs:comment xml:lang="OWLManchester">platform:implementsInterface some JavaxSecurityCertAPI</rdfs:comment>
	</owl:Class>
	<owl:Class rdf:about="&android-1_6;JavaxCryptoClassLibrary">
		<owl:equivalentClass rdf:resource="&j2se-5_0;JavaxCryptoClassLibrary"/>
		<owl:equivalentClass rdf:resource="&android-1_5;JavaxCryptoClassLibrary"/>
		<rdfs:subClassOf rdf:resource="&java;JavaClassLibrary"/>
		<rdfs:comment xml:lang="en">JavaLibrary implementing the javax.crypto package for Android 1.6</rdfs:comment>
		<rdfs:comment xml:lang="OWLManchester">platform:implementsInterface some JavaxCryptoAPI</rdfs:comment>
	</owl:Class>
	<owl:Class rdf:about="&android-1_6;JavaxCryptoInterfacesClassLibrary">
		<owl:equivalentClass rdf:resource="&j2se-5_0;JavaxCryptoInterfacesClassLibrary"/>
		<owl:equivalentClass rdf:resource="&android-1_5;JavaxCryptoInterfacesClassLibrary"/>
		<rdfs:subClassOf rdf:resource="&java;JavaClassLibrary"/>
		<rdfs:comment xml:lang="en">JavaLibrary implementing the javax.crypto.interfaces package for Android 1.6</rdfs:comment>
		<rdfs:comment xml:lang="OWLManchester">platform:implementsInterface some JavaxCryptoInterfacesAPI</rdfs:comment>
	</owl:Class>
	<owl:Class rdf:about="&android-1_6;JavaxCryptoSpecClassLibrary">
		<owl:equivalentClass rdf:resource="&j2se-5_0;JavaxCryptoSpecClassLibrary"/>
		<owl:equivalentClass rdf:resource="&android-1_5;JavaxCryptoSpecClassLibrary"/>
		<rdfs:subClassOf rdf:resource="&java;JavaClassLibrary"/>
		<rdfs:comment xml:lang="en">JavaLibrary implementing the javax.crypto.spec package for Android 1.6</rdfs:comment>
		<rdfs:comment xml:lang="OWLManchester">platform:implementsInterface some JavaxCryptoSpecAPI</rdfs:comment>
	</owl:Class>
	<owl:Class rdf:about="&android-1_6;JavaxSqlClassLibrary">
		<owl:equivalentClass rdf:resource="&android-1_5;JavaxSqlClassLibrary"/>
		<rdfs:subClassOf rdf:resource="&java;JavaClassLibrary"/>
		<rdfs:comment xml:lang="en">JavaLibrary implementing the javax.sql package for Android 1.6</rdfs:comment>
		<rdfs:comment xml:lang="OWLManchester">platform:implementsInterface some JavaxSqlAPI</rdfs:comment>
	</owl:Class>
	<owl:Class rdf:about="&android-1_6;JavaxXmlClassLibrary">
		<owl:equivalentClass rdf:resource="&android-1_5;JavaxXmlClassLibrary"/>
		<rdfs:subClassOf rdf:resource="&j2se-5_0;JavaxXmlClassLibrary"/>
		<rdfs:comment xml:lang="en">JavaLibrary implementing the javax.xml package for Android 1.6</rdfs:comment>
		<rdfs:comment xml:lang="OWLManchester">platform:implementsInterface some JavaxXmlAPI</rdfs:comment>
	</owl:Class>
	<owl:Class rdf:about="&android-1_6;JavaxXmlParsersClassLibrary">
		<owl:equivalentClass rdf:resource="&android-1_5;JavaxXmlParsersClassLibrary"/>
		<rdfs:subClassOf rdf:resource="&java;JavaClassLibrary"/>
		<rdfs:comment xml:lang="en">JavaLibrary implementing the javax.xml.parsers package for Android 1.6</rdfs:comment>
		<rdfs:comment xml:lang="OWLManchester">platform:implementsInterface some JavaxXmlParsersAPI</rdfs:comment>
	</owl:Class>
	<owl:Class rdf:about="&android-1_6;JunitFrameworkClassLibrary">
		<owl:equivalentClass rdf:resource="&android-1_5;JunitFrameworkClassLibrary"/>
		<rdfs:subClassOf rdf:resource="&java;JavaClassLibrary"/>
		<rdfs:comment xml:lang="en">JavaLibrary implementing the junit.framework package for Android 1.6</rdfs:comment>
		<rdfs:comment xml:lang="OWLManchester">platform:implementsInterface some JunitFrameworkAPI</rdfs:comment>
	</owl:Class>
	<owl:Class rdf:about="&android-1_6;JunitRunnerClassLibrary">
		<owl:equivalentClass rdf:resource="&android-1_5;JunitRunnerClassLibrary"/>
		<rdfs:subClassOf rdf:resource="&java;JavaClassLibrary"/>
		<rdfs:comment xml:lang="en">JavaLibrary implementing the junit.runner package for Android 1.6</rdfs:comment>
		<rdfs:comment xml:lang="OWLManchester">platform:implementsInterface some JunitRunnerAPI</rdfs:comment>
	</owl:Class>
	<owl:Class rdf:about="&android-1_6;DalvikAnnotationClassLibrary">
		<owl:equivalentClass rdf:resource="&android-1_5;DalvikAnnotationClassLibrary"/>
		<rdfs:subClassOf rdf:resource="&java;JavaClassLibrary"/>
		<rdfs:comment xml:lang="en">JavaLibrary implementing the dalvik.annotation package for Android 1.6</rdfs:comment>
		<rdfs:comment xml:lang="OWLManchester">platform:implementsInterface some DalvikAnnotationAPI</rdfs:comment>
	</owl:Class>
	<owl:Class rdf:about="&android-1_6;DalvikBytecodeClassLibrary">
		<owl:equivalentClass rdf:resource="&android-1_5;DalvikBytecodeClassLibrary"/>
		<rdfs:subClassOf rdf:resource="&java;JavaClassLibrary"/>
		<rdfs:comment xml:lang="en">JavaLibrary implementing the dalvik.bytecode package for Android 1.6</rdfs:comment>
		<rdfs:comment xml:lang="OWLManchester">platform:implementsInterface some DalvikBytecodeAPI</rdfs:comment>
	</owl:Class>
	<owl:Class rdf:about="&android-1_6;DalvikSystemClassLibrary">
		<owl:equivalentClass rdf:resource="&android-1_5;DalvikSystemClassLibrary"/>
		<rdfs:subClassOf rdf:resource="&java;JavaClassLibrary"/>
		<rdfs:comment xml:lang="en">JavaLibrary implementing the dalvik.system package for Android 1.6</rdfs:comment>
		<rdfs:comment xml:lang="OWLManchester">platform:implementsInterface some DalvikSystemAPI</rdfs:comment>
	</owl:Class>
</rdf:RDF>
