<?xml version="1.0" encoding="ISO-8859-1"?>
<!DOCTYPE rdf:RDF [
	<!ENTITY j2me-pp-1_1 "http://soft.vub.ac.be/platformkit/2010/1/j2me-pp-1_1.owl#">
	<!ENTITY xsd "http://www.w3.org/2001/XMLSchema#">
	<!ENTITY j2me-pp-1_0 "http://soft.vub.ac.be/platformkit/2010/1/j2me-pp-1_0.owl#">
	<!ENTITY platform "http://localhost/~dennis/platformkit/2010_1/platform.owl#">
	<!ENTITY ns_19 "http://localhost/~dennis/platformkit/2010_1/">
	<!ENTITY java "http://localhost/~dennis/platformkit/2010_1/java.owl#">
	<!ENTITY j2se-1_3 "http://soft.vub.ac.be/platformkit/2010/1/j2se-1_3.owl#">
	<!ENTITY isa "http://localhost/~dennis/platformkit/2010_1/isa.owl#">
	<!ENTITY rdf "http://www.w3.org/1999/02/22-rdf-syntax-ns#">
	<!ENTITY rdfs "http://www.w3.org/2000/01/rdf-schema#">
	<!ENTITY owl "http://www.w3.org/2002/07/owl#">
]>
<rdf:RDF
	 xmlns:j2me-pp-1_1="&j2me-pp-1_1;"
	 xmlns:xsd="&xsd;"
	 xmlns:j2me-pp-1_0="&j2me-pp-1_0;"
	 xmlns:platform="&platform;"
	 xmlns:ns_19="&ns_19;"
	 xmlns:java="&java;"
	 xmlns:j2se-1_3="&j2se-1_3;"
	 xmlns:isa="&isa;"
	 xmlns:rdf="&rdf;"
	 xmlns:rdfs="&rdfs;"
	 xmlns:owl="&owl;"
>

	<owl:Ontology rdf:about="http://soft.vub.ac.be/platformkit/2010/1/j2me-pp-1_1.owl#">
		<owl:versionInfo>$Id: UML2ToPackageAPIOntology.atl 8082 2010-03-18 21:11:00Z dwagelaa $</owl:versionInfo>
		<owl:imports rdf:resource="http://localhost/~dennis/platformkit/2010_1/platform.owl"/>
		<owl:imports rdf:resource="http://localhost/~dennis/platformkit/2010_1/java.owl"/>
		<owl:imports rdf:resource="http://soft.vub.ac.be/platformkit/2010/1/j2se-1_3.owl#"/>
		<owl:imports rdf:resource="http://localhost/~dennis/platformkit/2010_1/isa.owl"/>
		<owl:imports rdf:resource="http://soft.vub.ac.be/platformkit/2010/1/j2me-pp-1_0.owl#"/>
		<rdfs:comment xml:lang="en">Generated by [UML2ToSimplifiedPackageAPIOntology.atl 8080 2010-03-18 10:46:40Z dwagelaa], [UML2ToPackageAPIOntology.atl 8082 2010-03-18 21:11:00Z dwagelaa], [UML2ToAPIOntology.atl 8082 2010-03-18 21:11:00Z dwagelaa], and [UML2Comparison.atl 8082 2010-03-18 21:11:00Z dwagelaa]</rdfs:comment>
		<rdfs:comment>Dennis Wagelaar &lt;dennis.wagelaar@vub.ac.be&gt;</rdfs:comment>
		<rdfs:comment xml:lang="en">&#169; 2010, Vrije Universiteit Brussel. All rights reserved.</rdfs:comment>
		<rdfs:label xml:lang="en">J2ME PP 1.1</rdfs:label>
	</owl:Ontology>
	<owl:Class rdf:about="&j2me-pp-1_1;J2MEPP1_1API">
		<rdfs:subClassOf rdf:resource="&j2me-pp-1_1;JavaIoAPI"/>
		<rdfs:subClassOf rdf:resource="&j2me-pp-1_1;JavaLangAPI"/>
		<rdfs:subClassOf rdf:resource="&j2me-pp-1_1;JavaLangRefAPI"/>
		<rdfs:subClassOf rdf:resource="&j2me-pp-1_1;JavaLangReflectAPI"/>
		<rdfs:subClassOf rdf:resource="&j2me-pp-1_1;JavaSecurityAPI"/>
		<rdfs:subClassOf rdf:resource="&j2me-pp-1_1;JavaSecurityCertAPI"/>
		<rdfs:subClassOf rdf:resource="&j2me-pp-1_1;JavaSecurityInterfacesAPI"/>
		<rdfs:subClassOf rdf:resource="&j2me-pp-1_1;JavaSecuritySpecAPI"/>
		<rdfs:subClassOf rdf:resource="&j2me-pp-1_1;JavaSecurityAclAPI"/>
		<rdfs:subClassOf rdf:resource="&j2me-pp-1_1;JavaNetAPI"/>
		<rdfs:subClassOf rdf:resource="&j2me-pp-1_1;JavaUtilAPI"/>
		<rdfs:subClassOf rdf:resource="&j2me-pp-1_1;JavaUtilJarAPI"/>
		<rdfs:subClassOf rdf:resource="&j2me-pp-1_1;JavaUtilZipAPI"/>
		<rdfs:subClassOf rdf:resource="&j2me-pp-1_1;JavaMathAPI"/>
		<rdfs:subClassOf rdf:resource="&j2me-pp-1_1;JavaTextAPI"/>
		<rdfs:subClassOf rdf:resource="&j2me-pp-1_1;JavaAwtAPI"/>
		<rdfs:subClassOf rdf:resource="&j2me-pp-1_1;JavaAwtImAPI"/>
		<rdfs:subClassOf rdf:resource="&j2me-pp-1_1;JavaAwtFontAPI"/>
		<rdfs:subClassOf rdf:resource="&j2me-pp-1_1;JavaAwtEventAPI"/>
		<rdfs:subClassOf rdf:resource="&j2me-pp-1_1;JavaAwtImageAPI"/>
		<rdfs:subClassOf rdf:resource="&j2me-pp-1_1;JavaAwtColorAPI"/>
		<rdfs:subClassOf rdf:resource="&j2me-pp-1_1;JavaAwtDatatransferAPI"/>
		<rdfs:subClassOf rdf:resource="&j2me-pp-1_1;JavaBeansAPI"/>
		<rdfs:subClassOf rdf:resource="&j2me-pp-1_1;JavaRmiAPI"/>
		<rdfs:subClassOf rdf:resource="&j2me-pp-1_1;JavaRmiRegistryAPI"/>
		<rdfs:subClassOf rdf:resource="&j2me-pp-1_1;JavaAppletAPI"/>
		<rdfs:subClassOf rdf:resource="&j2me-pp-1_1;JavaxSecurityAuthX500API"/>
		<rdfs:subClassOf rdf:resource="&j2me-pp-1_1;JavaxMicroeditionIoAPI"/>
		<rdfs:subClassOf rdf:resource="&j2me-pp-1_1;JavaxMicroeditionPkiAPI"/>
		<rdfs:subClassOf rdf:resource="&j2me-pp-1_1;JavaxMicroeditionXletAPI"/>
		<rdfs:subClassOf rdf:resource="&j2me-pp-1_1;JavaxMicroeditionXletIxcAPI"/>
		<rdfs:comment xml:lang="en">J2ME PP 1.1 API</rdfs:comment>
		<rdfs:comment xml:lang="OWLManchester">platform:comprisesInterfacePart some JavaIo and platform:comprisesInterfacePart some JavaLang and platform:comprisesInterfacePart some JavaLangRef and platform:comprisesInterfacePart some JavaLangReflect and platform:comprisesInterfacePart some JavaSecurity and platform:comprisesInterfacePart some JavaSecurityCert and platform:comprisesInterfacePart some JavaSecurityInterfaces and platform:comprisesInterfacePart some JavaSecuritySpec and platform:comprisesInterfacePart some JavaSecurityAcl and platform:comprisesInterfacePart some JavaNet and platform:comprisesInterfacePart some JavaUtil and platform:comprisesInterfacePart some JavaUtilJar and platform:comprisesInterfacePart some JavaUtilZip and platform:comprisesInterfacePart some JavaMath and platform:comprisesInterfacePart some JavaText and platform:comprisesInterfacePart some JavaAwt and platform:comprisesInterfacePart some JavaAwtIm and platform:comprisesInterfacePart some JavaAwtFont and platform:comprisesInterfacePart some JavaAwtEvent and platform:comprisesInterfacePart some JavaAwtImage and platform:comprisesInterfacePart some JavaAwtColor and platform:comprisesInterfacePart some JavaAwtDatatransfer and platform:comprisesInterfacePart some JavaBeans and platform:comprisesInterfacePart some JavaRmi and platform:comprisesInterfacePart some JavaRmiRegistry and platform:comprisesInterfacePart some JavaApplet and platform:comprisesInterfacePart some JavaxSecurityAuthX500 and platform:comprisesInterfacePart some JavaxMicroeditionIo and platform:comprisesInterfacePart some JavaxMicroeditionPki and platform:comprisesInterfacePart some JavaxMicroeditionXlet and platform:comprisesInterfacePart some JavaxMicroeditionXletIxc</rdfs:comment>
	</owl:Class>
	<owl:Class rdf:about="&j2me-pp-1_1;J2MEPP1_1ClassLibrary">
		<rdfs:subClassOf rdf:resource="&j2me-pp-1_1;JavaIoClassLibrary"/>
		<rdfs:subClassOf rdf:resource="&j2me-pp-1_1;JavaLangClassLibrary"/>
		<rdfs:subClassOf rdf:resource="&j2me-pp-1_1;JavaLangRefClassLibrary"/>
		<rdfs:subClassOf rdf:resource="&j2me-pp-1_1;JavaLangReflectClassLibrary"/>
		<rdfs:subClassOf rdf:resource="&j2me-pp-1_1;JavaSecurityClassLibrary"/>
		<rdfs:subClassOf rdf:resource="&j2me-pp-1_1;JavaSecurityCertClassLibrary"/>
		<rdfs:subClassOf rdf:resource="&j2me-pp-1_1;JavaSecurityInterfacesClassLibrary"/>
		<rdfs:subClassOf rdf:resource="&j2me-pp-1_1;JavaSecuritySpecClassLibrary"/>
		<rdfs:subClassOf rdf:resource="&j2me-pp-1_1;JavaSecurityAclClassLibrary"/>
		<rdfs:subClassOf rdf:resource="&j2me-pp-1_1;JavaNetClassLibrary"/>
		<rdfs:subClassOf rdf:resource="&j2me-pp-1_1;JavaUtilClassLibrary"/>
		<rdfs:subClassOf rdf:resource="&j2me-pp-1_1;JavaUtilJarClassLibrary"/>
		<rdfs:subClassOf rdf:resource="&j2me-pp-1_1;JavaUtilZipClassLibrary"/>
		<rdfs:subClassOf rdf:resource="&j2me-pp-1_1;JavaMathClassLibrary"/>
		<rdfs:subClassOf rdf:resource="&j2me-pp-1_1;JavaTextClassLibrary"/>
		<rdfs:subClassOf rdf:resource="&j2me-pp-1_1;JavaAwtClassLibrary"/>
		<rdfs:subClassOf rdf:resource="&j2me-pp-1_1;JavaAwtImClassLibrary"/>
		<rdfs:subClassOf rdf:resource="&j2me-pp-1_1;JavaAwtFontClassLibrary"/>
		<rdfs:subClassOf rdf:resource="&j2me-pp-1_1;JavaAwtEventClassLibrary"/>
		<rdfs:subClassOf rdf:resource="&j2me-pp-1_1;JavaAwtImageClassLibrary"/>
		<rdfs:subClassOf rdf:resource="&j2me-pp-1_1;JavaAwtColorClassLibrary"/>
		<rdfs:subClassOf rdf:resource="&j2me-pp-1_1;JavaAwtDatatransferClassLibrary"/>
		<rdfs:subClassOf rdf:resource="&j2me-pp-1_1;JavaBeansClassLibrary"/>
		<rdfs:subClassOf rdf:resource="&j2me-pp-1_1;JavaRmiClassLibrary"/>
		<rdfs:subClassOf rdf:resource="&j2me-pp-1_1;JavaRmiRegistryClassLibrary"/>
		<rdfs:subClassOf rdf:resource="&j2me-pp-1_1;JavaAppletClassLibrary"/>
		<rdfs:subClassOf rdf:resource="&j2me-pp-1_1;JavaxSecurityAuthX500ClassLibrary"/>
		<rdfs:subClassOf rdf:resource="&j2me-pp-1_1;JavaxMicroeditionIoClassLibrary"/>
		<rdfs:subClassOf rdf:resource="&j2me-pp-1_1;JavaxMicroeditionPkiClassLibrary"/>
		<rdfs:subClassOf rdf:resource="&j2me-pp-1_1;JavaxMicroeditionXletClassLibrary"/>
		<rdfs:subClassOf rdf:resource="&j2me-pp-1_1;JavaxMicroeditionXletIxcClassLibrary"/>
		<rdfs:comment xml:lang="en">Java class library implementing the J2ME PP 1.1 API</rdfs:comment>
		<rdfs:comment xml:lang="OWLManchester">platform:implementsInterface some J2MEPP1_1API</rdfs:comment>
	</owl:Class>
	<owl:Class rdf:about="&j2me-pp-1_1;J2MEPP1_1BytecodeFormat">
		<rdfs:subClassOf rdf:resource="&j2me-pp-1_0;J2MEPP1_0BytecodeFormat"/>
		<rdfs:subClassOf rdf:resource="&j2se-1_3;J2SE1_3BytecodeFormat"/>
		<rdfs:comment xml:lang="en">J2ME PP 1.1 bytecode format</rdfs:comment>
		<rdfs:comment xml:lang="OWLManchester">java:majorVersionNumber some xsd:integer[>="48"^^xsd:integer] and java:preverified value false</rdfs:comment>
	</owl:Class>
	<j2me-pp-1_1:J2MEPP1_1BytecodeFormat rdf:about="&j2me-pp-1_1;theJ2MEPP1_1BytecodeFormat">
		<java:preverified rdf:datatype="http://www.w3.org/2001/XMLSchema#boolean">false</java:preverified>
		<java:minorVersionNumber rdf:datatype="http://www.w3.org/2001/XMLSchema#integer">0</java:minorVersionNumber>
		<java:majorVersionNumber rdf:datatype="http://www.w3.org/2001/XMLSchema#integer">48</java:majorVersionNumber>
	</j2me-pp-1_1:J2MEPP1_1BytecodeFormat>
	<j2me-pp-1_1:J2MEPP1_1API rdf:about="&j2me-pp-1_1;theJ2MEPP1_1API">
		<platform:comprisesInterfacePart rdf:resource="&j2me-pp-1_1;theJavaxMicroeditionXletIxcPart"/>
		<platform:comprisesInterfacePart rdf:resource="&j2me-pp-1_1;theJavaxMicroeditionXletPart"/>
		<platform:comprisesInterfacePart rdf:resource="&j2me-pp-1_1;theJavaxMicroeditionPkiPart"/>
		<platform:comprisesInterfacePart rdf:resource="&j2me-pp-1_1;theJavaxMicroeditionIoPart"/>
		<platform:comprisesInterfacePart rdf:resource="&j2me-pp-1_1;theJavaxSecurityAuthX500Part"/>
		<platform:comprisesInterfacePart rdf:resource="&j2me-pp-1_1;theJavaAppletPart"/>
		<platform:comprisesInterfacePart rdf:resource="&j2me-pp-1_1;theJavaRmiRegistryPart"/>
		<platform:comprisesInterfacePart rdf:resource="&j2me-pp-1_1;theJavaRmiPart"/>
		<platform:comprisesInterfacePart rdf:resource="&j2me-pp-1_1;theJavaBeansPart"/>
		<platform:comprisesInterfacePart rdf:resource="&j2me-pp-1_1;theJavaAwtDatatransferPart"/>
		<platform:comprisesInterfacePart rdf:resource="&j2me-pp-1_1;theJavaAwtColorPart"/>
		<platform:comprisesInterfacePart rdf:resource="&j2me-pp-1_1;theJavaAwtImagePart"/>
		<platform:comprisesInterfacePart rdf:resource="&j2me-pp-1_1;theJavaAwtEventPart"/>
		<platform:comprisesInterfacePart rdf:resource="&j2me-pp-1_1;theJavaAwtFontPart"/>
		<platform:comprisesInterfacePart rdf:resource="&j2me-pp-1_1;theJavaAwtImPart"/>
		<platform:comprisesInterfacePart rdf:resource="&j2me-pp-1_1;theJavaAwtPart"/>
		<platform:comprisesInterfacePart rdf:resource="&j2me-pp-1_1;theJavaTextPart"/>
		<platform:comprisesInterfacePart rdf:resource="&j2me-pp-1_1;theJavaMathPart"/>
		<platform:comprisesInterfacePart rdf:resource="&j2me-pp-1_1;theJavaUtilZipPart"/>
		<platform:comprisesInterfacePart rdf:resource="&j2me-pp-1_1;theJavaUtilJarPart"/>
		<platform:comprisesInterfacePart rdf:resource="&j2me-pp-1_1;theJavaUtilPart"/>
		<platform:comprisesInterfacePart rdf:resource="&j2me-pp-1_1;theJavaNetPart"/>
		<platform:comprisesInterfacePart rdf:resource="&j2me-pp-1_1;theJavaSecurityAclPart"/>
		<platform:comprisesInterfacePart rdf:resource="&j2me-pp-1_1;theJavaSecuritySpecPart"/>
		<platform:comprisesInterfacePart rdf:resource="&j2me-pp-1_1;theJavaSecurityInterfacesPart"/>
		<platform:comprisesInterfacePart rdf:resource="&j2me-pp-1_1;theJavaSecurityCertPart"/>
		<platform:comprisesInterfacePart rdf:resource="&j2me-pp-1_1;theJavaSecurityPart"/>
		<platform:comprisesInterfacePart rdf:resource="&j2me-pp-1_1;theJavaLangReflectPart"/>
		<platform:comprisesInterfacePart rdf:resource="&j2me-pp-1_1;theJavaLangRefPart"/>
		<platform:comprisesInterfacePart rdf:resource="&j2me-pp-1_1;theJavaLangPart"/>
		<platform:comprisesInterfacePart rdf:resource="&j2me-pp-1_1;theJavaIoPart"/>
	</j2me-pp-1_1:J2MEPP1_1API>
	<owl:Class rdf:about="&j2me-pp-1_1;J2MEPP1_1VM">
		<owl:equivalentClass>
			<owl:Restriction>
				<owl:onProperty rdf:resource="&platform;implementsInterface"/>
				<owl:someValuesFrom rdf:resource="&j2me-pp-1_1;J2MEPP1_1BytecodeFormat"/>
			</owl:Restriction>
		</owl:equivalentClass>
		<rdfs:subClassOf rdf:resource="&java;JavaVM"/>
		<rdfs:comment xml:lang="en">J2ME PP 1.1 virtual machine</rdfs:comment>
	</owl:Class>
	<owl:Class rdf:about="&j2me-pp-1_1;J2MEPP1_1JRE">
		<owl:equivalentClass>
			<owl:Class >
				<owl:intersectionOf rdf:parseType="Collection">
					<owl:Restriction>
						<owl:onProperty rdf:resource="&platform;providesFeature"/>
						<owl:someValuesFrom rdf:resource="&j2me-pp-1_1;J2MEPP1_1ClassLibrary"/>
					</owl:Restriction>
					<owl:Restriction>
						<owl:onProperty rdf:resource="&platform;providesFeature"/>
						<owl:someValuesFrom rdf:resource="&j2me-pp-1_1;J2MEPP1_1VM"/>
					</owl:Restriction>
				</owl:intersectionOf>
			</owl:Class>
		</owl:equivalentClass>
		<rdfs:subClassOf rdf:resource="&java;JRE"/>
		<rdfs:comment xml:lang="en">J2ME PP 1.1 Java Runtime Environment</rdfs:comment>
	</owl:Class>
	<owl:Class rdf:about="&j2me-pp-1_1;JavaIo">
		<rdfs:subClassOf rdf:resource="&j2me-pp-1_0;JavaIo"/>
		<rdfs:seeAlso rdf:resource="&j2me-pp-1_1;JavaLang"/>
		<rdfs:seeAlso rdf:resource="&j2me-pp-1_1;JavaNet"/>
		<rdfs:seeAlso rdf:resource="&j2me-pp-1_1;JavaUtil"/>
		<rdfs:seeAlso rdf:resource="&j2me-pp-1_1;JavaSecurity"/>
		<rdfs:comment xml:lang="en">Java API part implementing the java.io package for J2ME PP 1.1</rdfs:comment>
	</owl:Class>
	<owl:Class rdf:about="&j2me-pp-1_1;JavaLang">
		<rdfs:subClassOf rdf:resource="&j2me-pp-1_0;JavaLang"/>
		<rdfs:seeAlso rdf:resource="&j2me-pp-1_1;JavaNet"/>
		<rdfs:seeAlso rdf:resource="&j2me-pp-1_1;JavaLangReflect"/>
		<rdfs:seeAlso rdf:resource="&j2me-pp-1_1;JavaUtil"/>
		<rdfs:seeAlso rdf:resource="&j2me-pp-1_1;JavaIo"/>
		<rdfs:seeAlso rdf:resource="&j2me-pp-1_1;JavaSecurity"/>
		<rdfs:comment xml:lang="en">Java API part implementing the java.lang package for J2ME PP 1.1</rdfs:comment>
	</owl:Class>
	<owl:Class rdf:about="&j2me-pp-1_1;JavaLangRef">
		<owl:equivalentClass rdf:resource="&j2me-pp-1_0;JavaLangRef"/>
		<owl:equivalentClass rdf:resource="&j2se-1_3;JavaLangRef"/>
		<rdfs:subClassOf rdf:resource="&java;JavaAPIPart"/>
		<rdfs:seeAlso rdf:resource="&j2me-pp-1_1;JavaLang"/>
		<rdfs:comment xml:lang="en">Java API part implementing the java.lang.ref package for J2ME PP 1.1</rdfs:comment>
	</owl:Class>
	<owl:Class rdf:about="&j2me-pp-1_1;JavaLangReflect">
		<rdfs:subClassOf rdf:resource="&j2me-pp-1_0;JavaLangReflect"/>
		<rdfs:subClassOf rdf:resource="&j2se-1_3;JavaLangReflect"/>
		<rdfs:seeAlso rdf:resource="&j2me-pp-1_1;JavaLang"/>
		<rdfs:seeAlso rdf:resource="&j2me-pp-1_1;JavaIo"/>
		<rdfs:seeAlso rdf:resource="&j2me-pp-1_1;JavaSecurity"/>
		<rdfs:comment xml:lang="en">Java API part implementing the java.lang.reflect package for J2ME PP 1.1</rdfs:comment>
	</owl:Class>
	<owl:Class rdf:about="&j2me-pp-1_1;JavaSecurity">
		<rdfs:subClassOf rdf:resource="&j2me-pp-1_0;JavaSecurity"/>
		<rdfs:seeAlso rdf:resource="&j2me-pp-1_1;JavaLang"/>
		<rdfs:seeAlso rdf:resource="&j2me-pp-1_1;JavaSecuritySpec"/>
		<rdfs:seeAlso rdf:resource="&j2me-pp-1_1;JavaUtil"/>
		<rdfs:seeAlso rdf:resource="&j2me-pp-1_1;JavaIo"/>
		<rdfs:seeAlso rdf:resource="&j2me-pp-1_1;JavaNet"/>
		<rdfs:seeAlso rdf:resource="&j2me-pp-1_1;JavaSecurityCert"/>
		<rdfs:comment xml:lang="en">Java API part implementing the java.security package for J2ME PP 1.1</rdfs:comment>
	</owl:Class>
	<owl:Class rdf:about="&j2me-pp-1_1;JavaSecurityCert">
		<rdfs:subClassOf rdf:resource="&j2me-pp-1_0;JavaSecurityCert"/>
		<rdfs:subClassOf rdf:resource="&j2se-1_3;JavaSecurityCert"/>
		<rdfs:seeAlso rdf:resource="&j2me-pp-1_1;JavaLang"/>
		<rdfs:seeAlso rdf:resource="&j2me-pp-1_1;JavaxSecurityAuthX500"/>
		<rdfs:seeAlso rdf:resource="&j2me-pp-1_1;JavaMath"/>
		<rdfs:seeAlso rdf:resource="&j2me-pp-1_1;JavaUtil"/>
		<rdfs:seeAlso rdf:resource="&j2me-pp-1_1;JavaIo"/>
		<rdfs:seeAlso rdf:resource="&j2me-pp-1_1;JavaSecurity"/>
		<rdfs:comment xml:lang="en">Java API part implementing the java.security.cert package for J2ME PP 1.1</rdfs:comment>
	</owl:Class>
	<owl:Class rdf:about="&j2me-pp-1_1;JavaSecurityInterfaces">
		<owl:equivalentClass rdf:resource="&j2me-pp-1_0;JavaSecurityInterfaces"/>
		<owl:equivalentClass rdf:resource="&j2se-1_3;JavaSecurityInterfaces"/>
		<rdfs:subClassOf rdf:resource="&java;JavaAPIPart"/>
		<rdfs:seeAlso rdf:resource="&j2me-pp-1_1;JavaMath"/>
		<rdfs:seeAlso rdf:resource="&j2me-pp-1_1;JavaSecurity"/>
		<rdfs:comment xml:lang="en">Java API part implementing the java.security.interfaces package for J2ME PP 1.1</rdfs:comment>
	</owl:Class>
	<owl:Class rdf:about="&j2me-pp-1_1;JavaSecuritySpec">
		<rdfs:subClassOf rdf:resource="&j2me-pp-1_0;JavaSecuritySpec"/>
		<rdfs:subClassOf rdf:resource="&j2se-1_3;JavaSecuritySpec"/>
		<rdfs:seeAlso rdf:resource="&j2me-pp-1_1;JavaLang"/>
		<rdfs:seeAlso rdf:resource="&j2me-pp-1_1;JavaMath"/>
		<rdfs:seeAlso rdf:resource="&j2me-pp-1_1;JavaSecurityInterfaces"/>
		<rdfs:seeAlso rdf:resource="&j2me-pp-1_1;JavaSecurity"/>
		<rdfs:comment xml:lang="en">Java API part implementing the java.security.spec package for J2ME PP 1.1</rdfs:comment>
	</owl:Class>
	<owl:Class rdf:about="&j2me-pp-1_1;JavaSecurityAcl">
		<rdfs:subClassOf rdf:resource="&j2me-pp-1_0;JavaSecurityAcl"/>
		<rdfs:subClassOf rdf:resource="&j2se-1_3;JavaSecurityAcl"/>
		<rdfs:seeAlso rdf:resource="&j2me-pp-1_1;JavaLang"/>
		<rdfs:seeAlso rdf:resource="&j2me-pp-1_1;JavaUtil"/>
		<rdfs:seeAlso rdf:resource="&j2me-pp-1_1;JavaSecurity"/>
		<rdfs:comment xml:lang="en">Java API part implementing the java.security.acl package for J2ME PP 1.1</rdfs:comment>
	</owl:Class>
	<owl:Class rdf:about="&j2me-pp-1_1;JavaNet">
		<rdfs:subClassOf rdf:resource="&j2me-pp-1_0;JavaNet"/>
		<rdfs:seeAlso rdf:resource="&j2me-pp-1_1;JavaLang"/>
		<rdfs:seeAlso rdf:resource="&j2me-pp-1_1;JavaUtil"/>
		<rdfs:seeAlso rdf:resource="&j2me-pp-1_1;JavaIo"/>
		<rdfs:seeAlso rdf:resource="&j2me-pp-1_1;JavaUtilJar"/>
		<rdfs:seeAlso rdf:resource="&j2me-pp-1_1;JavaSecurity"/>
		<rdfs:comment xml:lang="en">Java API part implementing the java.net package for J2ME PP 1.1</rdfs:comment>
	</owl:Class>
	<owl:Class rdf:about="&j2me-pp-1_1;JavaUtil">
		<rdfs:subClassOf rdf:resource="&j2me-pp-1_0;JavaUtil"/>
		<rdfs:seeAlso rdf:resource="&j2me-pp-1_1;JavaLang"/>
		<rdfs:seeAlso rdf:resource="&j2me-pp-1_1;JavaIo"/>
		<rdfs:seeAlso rdf:resource="&j2me-pp-1_1;JavaSecurity"/>
		<rdfs:comment xml:lang="en">Java API part implementing the java.util package for J2ME PP 1.1</rdfs:comment>
	</owl:Class>
	<owl:Class rdf:about="&j2me-pp-1_1;JavaUtilJar">
		<rdfs:subClassOf rdf:resource="&j2me-pp-1_0;JavaUtilJar"/>
		<rdfs:subClassOf rdf:resource="&j2se-1_3;JavaUtilJar"/>
		<rdfs:seeAlso rdf:resource="&j2me-pp-1_1;JavaLang"/>
		<rdfs:seeAlso rdf:resource="&j2me-pp-1_1;JavaUtilZip"/>
		<rdfs:seeAlso rdf:resource="&j2me-pp-1_1;JavaUtil"/>
		<rdfs:seeAlso rdf:resource="&j2me-pp-1_1;JavaIo"/>
		<rdfs:comment xml:lang="en">Java API part implementing the java.util.jar package for J2ME PP 1.1</rdfs:comment>
	</owl:Class>
	<owl:Class rdf:about="&j2me-pp-1_1;JavaUtilZip">
		<rdfs:subClassOf rdf:resource="&j2me-pp-1_0;JavaUtilZip"/>
		<rdfs:subClassOf rdf:resource="&j2se-1_3;JavaUtilZip"/>
		<rdfs:seeAlso rdf:resource="&j2me-pp-1_1;JavaLang"/>
		<rdfs:seeAlso rdf:resource="&j2me-pp-1_1;JavaUtil"/>
		<rdfs:seeAlso rdf:resource="&j2me-pp-1_1;JavaIo"/>
		<rdfs:comment xml:lang="en">Java API part implementing the java.util.zip package for J2ME PP 1.1</rdfs:comment>
	</owl:Class>
	<owl:Class rdf:about="&j2me-pp-1_1;JavaMath">
		<owl:equivalentClass rdf:resource="&j2me-pp-1_0;JavaMath"/>
		<owl:equivalentClass rdf:resource="&j2se-1_3;JavaMath"/>
		<rdfs:subClassOf rdf:resource="&java;JavaAPIPart"/>
		<rdfs:seeAlso rdf:resource="&j2me-pp-1_1;JavaLang"/>
		<rdfs:seeAlso rdf:resource="&j2me-pp-1_1;JavaUtil"/>
		<rdfs:comment xml:lang="en">Java API part implementing the java.math package for J2ME PP 1.1</rdfs:comment>
	</owl:Class>
	<owl:Class rdf:about="&j2me-pp-1_1;JavaText">
		<rdfs:subClassOf rdf:resource="&j2me-pp-1_0;JavaText"/>
		<rdfs:subClassOf rdf:resource="&j2se-1_3;JavaText"/>
		<rdfs:seeAlso rdf:resource="&j2me-pp-1_1;JavaLang"/>
		<rdfs:seeAlso rdf:resource="&j2me-pp-1_1;JavaUtil"/>
		<rdfs:seeAlso rdf:resource="&j2me-pp-1_1;JavaIo"/>
		<rdfs:comment xml:lang="en">Java API part implementing the java.text package for J2ME PP 1.1</rdfs:comment>
	</owl:Class>
	<owl:Class rdf:about="&j2me-pp-1_1;JavaAwt">
		<rdfs:subClassOf rdf:resource="&j2me-pp-1_0;JavaAwt"/>
		<rdfs:seeAlso rdf:resource="&j2me-pp-1_1;JavaAwtDatatransfer"/>
		<rdfs:seeAlso rdf:resource="&j2me-pp-1_1;JavaBeans"/>
		<rdfs:seeAlso rdf:resource="&j2me-pp-1_1;JavaText"/>
		<rdfs:seeAlso rdf:resource="&j2me-pp-1_1;JavaUtil"/>
		<rdfs:seeAlso rdf:resource="&j2me-pp-1_1;JavaIo"/>
		<rdfs:seeAlso rdf:resource="&j2me-pp-1_1;JavaAwtEvent"/>
		<rdfs:seeAlso rdf:resource="&j2me-pp-1_1;JavaAwtIm"/>
		<rdfs:seeAlso rdf:resource="&j2me-pp-1_1;JavaLang"/>
		<rdfs:seeAlso rdf:resource="&j2me-pp-1_1;JavaAwtColor"/>
		<rdfs:seeAlso rdf:resource="&j2me-pp-1_1;JavaNet"/>
		<rdfs:seeAlso rdf:resource="&j2me-pp-1_1;JavaAwtImage"/>
		<rdfs:seeAlso rdf:resource="&j2me-pp-1_1;JavaSecurity"/>
		<rdfs:comment xml:lang="en">Java API part implementing the java.awt package for J2ME PP 1.1</rdfs:comment>
	</owl:Class>
	<owl:Class rdf:about="&j2me-pp-1_1;JavaAwtIm">
		<rdfs:subClassOf rdf:resource="&java;JavaAPIPart"/>
		<rdfs:seeAlso rdf:resource="&j2me-pp-1_1;JavaAwt"/>
		<rdfs:seeAlso rdf:resource="&j2me-pp-1_1;JavaLang"/>
		<rdfs:seeAlso rdf:resource="&j2me-pp-1_1;JavaUtil"/>
		<rdfs:seeAlso rdf:resource="&j2me-pp-1_1;JavaAwtFont"/>
		<rdfs:seeAlso rdf:resource="&j2me-pp-1_1;JavaText"/>
		<rdfs:comment xml:lang="en">Java API part implementing the java.awt.im package for J2ME PP 1.1</rdfs:comment>
	</owl:Class>
	<owl:Class rdf:about="&j2me-pp-1_1;JavaAwtFont">
		<rdfs:subClassOf rdf:resource="&java;JavaAPIPart"/>
		<rdfs:seeAlso rdf:resource="&j2me-pp-1_1;JavaLang"/>
		<rdfs:seeAlso rdf:resource="&j2me-pp-1_1;JavaText"/>
		<rdfs:comment xml:lang="en">Java API part implementing the java.awt.font package for J2ME PP 1.1</rdfs:comment>
	</owl:Class>
	<owl:Class rdf:about="&j2me-pp-1_1;JavaAwtEvent">
		<rdfs:subClassOf rdf:resource="&j2me-pp-1_0;JavaAwtEvent"/>
		<rdfs:seeAlso rdf:resource="&j2me-pp-1_1;JavaAwt"/>
		<rdfs:seeAlso rdf:resource="&j2me-pp-1_1;JavaLang"/>
		<rdfs:seeAlso rdf:resource="&j2me-pp-1_1;JavaAwtFont"/>
		<rdfs:seeAlso rdf:resource="&j2me-pp-1_1;JavaText"/>
		<rdfs:seeAlso rdf:resource="&j2me-pp-1_1;JavaUtil"/>
		<rdfs:comment xml:lang="en">Java API part implementing the java.awt.event package for J2ME PP 1.1</rdfs:comment>
	</owl:Class>
	<owl:Class rdf:about="&j2me-pp-1_1;JavaAwtImage">
		<rdfs:subClassOf rdf:resource="&j2me-pp-1_0;JavaAwtImage"/>
		<rdfs:seeAlso rdf:resource="&j2me-pp-1_1;JavaAwt"/>
		<rdfs:seeAlso rdf:resource="&j2me-pp-1_1;JavaAwtColor"/>
		<rdfs:seeAlso rdf:resource="&j2me-pp-1_1;JavaLang"/>
		<rdfs:seeAlso rdf:resource="&j2me-pp-1_1;JavaUtil"/>
		<rdfs:comment xml:lang="en">Java API part implementing the java.awt.image package for J2ME PP 1.1</rdfs:comment>
	</owl:Class>
	<owl:Class rdf:about="&j2me-pp-1_1;JavaAwtColor">
		<owl:equivalentClass rdf:resource="&j2me-pp-1_0;JavaAwtColor"/>
		<rdfs:subClassOf rdf:resource="&java;JavaAPIPart"/>
		<rdfs:seeAlso rdf:resource="&j2me-pp-1_1;JavaLang"/>
		<rdfs:seeAlso rdf:resource="&j2me-pp-1_1;JavaIo"/>
		<rdfs:comment xml:lang="en">Java API part implementing the java.awt.color package for J2ME PP 1.1</rdfs:comment>
	</owl:Class>
	<owl:Class rdf:about="&j2me-pp-1_1;JavaAwtDatatransfer">
		<rdfs:subClassOf rdf:resource="&j2me-pp-1_0;JavaAwtDatatransfer"/>
		<rdfs:seeAlso rdf:resource="&j2me-pp-1_1;JavaLang"/>
		<rdfs:seeAlso rdf:resource="&j2me-pp-1_1;JavaIo"/>
		<rdfs:comment xml:lang="en">Java API part implementing the java.awt.datatransfer package for J2ME PP 1.1</rdfs:comment>
	</owl:Class>
	<owl:Class rdf:about="&j2me-pp-1_1;JavaBeans">
		<rdfs:subClassOf rdf:resource="&j2me-pp-1_0;JavaBeans"/>
		<rdfs:seeAlso rdf:resource="&j2me-pp-1_1;JavaLang"/>
		<rdfs:seeAlso rdf:resource="&j2me-pp-1_1;JavaUtil"/>
		<rdfs:seeAlso rdf:resource="&j2me-pp-1_1;JavaIo"/>
		<rdfs:comment xml:lang="en">Java API part implementing the java.beans package for J2ME PP 1.1</rdfs:comment>
	</owl:Class>
	<owl:Class rdf:about="&j2me-pp-1_1;JavaRmi">
		<rdfs:subClassOf rdf:resource="&j2me-pp-1_0;JavaRmi"/>
		<rdfs:seeAlso rdf:resource="&j2me-pp-1_1;JavaLang"/>
		<rdfs:seeAlso rdf:resource="&j2me-pp-1_1;JavaIo"/>
		<rdfs:comment xml:lang="en">Java API part implementing the java.rmi package for J2ME PP 1.1</rdfs:comment>
	</owl:Class>
	<owl:Class rdf:about="&j2me-pp-1_1;JavaRmiRegistry">
		<owl:equivalentClass rdf:resource="&j2me-pp-1_0;JavaRmiRegistry"/>
		<rdfs:subClassOf rdf:resource="&java;JavaAPIPart"/>
		<rdfs:seeAlso rdf:resource="&j2me-pp-1_1;JavaLang"/>
		<rdfs:seeAlso rdf:resource="&j2me-pp-1_1;JavaRmi"/>
		<rdfs:comment xml:lang="en">Java API part implementing the java.rmi.registry package for J2ME PP 1.1</rdfs:comment>
	</owl:Class>
	<owl:Class rdf:about="&j2me-pp-1_1;JavaApplet">
		<rdfs:subClassOf rdf:resource="&j2me-pp-1_0;JavaApplet"/>
		<rdfs:seeAlso rdf:resource="&j2me-pp-1_1;JavaAwt"/>
		<rdfs:seeAlso rdf:resource="&j2me-pp-1_1;JavaLang"/>
		<rdfs:seeAlso rdf:resource="&j2me-pp-1_1;JavaUtil"/>
		<rdfs:seeAlso rdf:resource="&j2me-pp-1_1;JavaNet"/>
		<rdfs:comment xml:lang="en">Java API part implementing the java.applet package for J2ME PP 1.1</rdfs:comment>
	</owl:Class>
	<owl:Class rdf:about="&j2me-pp-1_1;JavaxSecurityAuthX500">
		<rdfs:subClassOf rdf:resource="&java;JavaAPIPart"/>
		<rdfs:seeAlso rdf:resource="&j2me-pp-1_1;JavaLang"/>
		<rdfs:seeAlso rdf:resource="&j2me-pp-1_1;JavaIo"/>
		<rdfs:seeAlso rdf:resource="&j2me-pp-1_1;JavaSecurity"/>
		<rdfs:comment xml:lang="en">Java API part implementing the javax.security.auth.x500 package for J2ME PP 1.1</rdfs:comment>
	</owl:Class>
	<owl:Class rdf:about="&j2me-pp-1_1;JavaxMicroeditionIo">
		<rdfs:subClassOf rdf:resource="&j2me-pp-1_0;JavaxMicroeditionIo"/>
		<rdfs:seeAlso rdf:resource="&j2me-pp-1_1;JavaLang"/>
		<rdfs:seeAlso rdf:resource="&j2me-pp-1_1;JavaIo"/>
		<rdfs:seeAlso rdf:resource="&j2me-pp-1_1;JavaxMicroeditionPki"/>
		<rdfs:comment xml:lang="en">Java API part implementing the javax.microedition.io package for J2ME PP 1.1</rdfs:comment>
	</owl:Class>
	<owl:Class rdf:about="&j2me-pp-1_1;JavaxMicroeditionPki">
		<rdfs:subClassOf rdf:resource="&java;JavaAPIPart"/>
		<rdfs:seeAlso rdf:resource="&j2me-pp-1_1;JavaLang"/>
		<rdfs:seeAlso rdf:resource="&j2me-pp-1_1;JavaIo"/>
		<rdfs:comment xml:lang="en">Java API part implementing the javax.microedition.pki package for J2ME PP 1.1</rdfs:comment>
	</owl:Class>
	<owl:Class rdf:about="&j2me-pp-1_1;JavaxMicroeditionXlet">
		<rdfs:subClassOf rdf:resource="&j2me-pp-1_0;JavaxMicroeditionXlet"/>
		<rdfs:seeAlso rdf:resource="&j2me-pp-1_1;JavaAwt"/>
		<rdfs:seeAlso rdf:resource="&j2me-pp-1_1;JavaLang"/>
		<rdfs:comment xml:lang="en">Java API part implementing the javax.microedition.xlet package for J2ME PP 1.1</rdfs:comment>
	</owl:Class>
	<owl:Class rdf:about="&j2me-pp-1_1;JavaxMicroeditionXletIxc">
		<rdfs:subClassOf rdf:resource="&j2me-pp-1_0;JavaxMicroeditionXletIxc"/>
		<rdfs:seeAlso rdf:resource="&j2me-pp-1_1;JavaxMicroeditionXlet"/>
		<rdfs:seeAlso rdf:resource="&j2me-pp-1_1;JavaLang"/>
		<rdfs:seeAlso rdf:resource="&j2me-pp-1_1;JavaRmi"/>
		<rdfs:seeAlso rdf:resource="&j2me-pp-1_1;JavaRmiRegistry"/>
		<rdfs:seeAlso rdf:resource="&j2me-pp-1_1;JavaSecurity"/>
		<rdfs:comment xml:lang="en">Java API part implementing the javax.microedition.xlet.ixc package for J2ME PP 1.1</rdfs:comment>
	</owl:Class>
	<owl:Class rdf:about="&j2me-pp-1_1;JavaIoAPI">
		<rdfs:subClassOf rdf:resource="&j2me-pp-1_0;JavaIoAPI"/>
		<rdfs:comment xml:lang="en">JavaLibrary implementing the java.io package for J2ME PP 1.1</rdfs:comment>
		<rdfs:comment xml:lang="OWLManchester">platform:comprisesInterfacePart some JavaIo</rdfs:comment>
	</owl:Class>
	<owl:Class rdf:about="&j2me-pp-1_1;JavaLangAPI">
		<rdfs:subClassOf rdf:resource="&j2me-pp-1_0;JavaLangAPI"/>
		<rdfs:comment xml:lang="en">JavaLibrary implementing the java.lang package for J2ME PP 1.1</rdfs:comment>
		<rdfs:comment xml:lang="OWLManchester">platform:comprisesInterfacePart some JavaLang</rdfs:comment>
	</owl:Class>
	<owl:Class rdf:about="&j2me-pp-1_1;JavaLangRefAPI">
		<owl:equivalentClass rdf:resource="&j2me-pp-1_0;JavaLangRefAPI"/>
		<owl:equivalentClass rdf:resource="&j2se-1_3;JavaLangRefAPI"/>
		<rdfs:subClassOf rdf:resource="&java;JavaAPI"/>
		<rdfs:comment xml:lang="en">JavaLibrary implementing the java.lang.ref package for J2ME PP 1.1</rdfs:comment>
		<rdfs:comment xml:lang="OWLManchester">platform:comprisesInterfacePart some JavaLangRef</rdfs:comment>
	</owl:Class>
	<owl:Class rdf:about="&j2me-pp-1_1;JavaLangReflectAPI">
		<rdfs:subClassOf rdf:resource="&j2me-pp-1_0;JavaLangReflectAPI"/>
		<rdfs:subClassOf rdf:resource="&j2se-1_3;JavaLangReflectAPI"/>
		<rdfs:comment xml:lang="en">JavaLibrary implementing the java.lang.reflect package for J2ME PP 1.1</rdfs:comment>
		<rdfs:comment xml:lang="OWLManchester">platform:comprisesInterfacePart some JavaLangReflect</rdfs:comment>
	</owl:Class>
	<owl:Class rdf:about="&j2me-pp-1_1;JavaSecurityAPI">
		<rdfs:subClassOf rdf:resource="&j2me-pp-1_0;JavaSecurityAPI"/>
		<rdfs:comment xml:lang="en">JavaLibrary implementing the java.security package for J2ME PP 1.1</rdfs:comment>
		<rdfs:comment xml:lang="OWLManchester">platform:comprisesInterfacePart some JavaSecurity</rdfs:comment>
	</owl:Class>
	<owl:Class rdf:about="&j2me-pp-1_1;JavaSecurityCertAPI">
		<rdfs:subClassOf rdf:resource="&j2me-pp-1_0;JavaSecurityCertAPI"/>
		<rdfs:subClassOf rdf:resource="&j2se-1_3;JavaSecurityCertAPI"/>
		<rdfs:comment xml:lang="en">JavaLibrary implementing the java.security.cert package for J2ME PP 1.1</rdfs:comment>
		<rdfs:comment xml:lang="OWLManchester">platform:comprisesInterfacePart some JavaSecurityCert</rdfs:comment>
	</owl:Class>
	<owl:Class rdf:about="&j2me-pp-1_1;JavaSecurityInterfacesAPI">
		<owl:equivalentClass rdf:resource="&j2me-pp-1_0;JavaSecurityInterfacesAPI"/>
		<owl:equivalentClass rdf:resource="&j2se-1_3;JavaSecurityInterfacesAPI"/>
		<rdfs:subClassOf rdf:resource="&java;JavaAPI"/>
		<rdfs:comment xml:lang="en">JavaLibrary implementing the java.security.interfaces package for J2ME PP 1.1</rdfs:comment>
		<rdfs:comment xml:lang="OWLManchester">platform:comprisesInterfacePart some JavaSecurityInterfaces</rdfs:comment>
	</owl:Class>
	<owl:Class rdf:about="&j2me-pp-1_1;JavaSecuritySpecAPI">
		<rdfs:subClassOf rdf:resource="&j2me-pp-1_0;JavaSecuritySpecAPI"/>
		<rdfs:subClassOf rdf:resource="&j2se-1_3;JavaSecuritySpecAPI"/>
		<rdfs:comment xml:lang="en">JavaLibrary implementing the java.security.spec package for J2ME PP 1.1</rdfs:comment>
		<rdfs:comment xml:lang="OWLManchester">platform:comprisesInterfacePart some JavaSecuritySpec</rdfs:comment>
	</owl:Class>
	<owl:Class rdf:about="&j2me-pp-1_1;JavaSecurityAclAPI">
		<rdfs:subClassOf rdf:resource="&j2me-pp-1_0;JavaSecurityAclAPI"/>
		<rdfs:subClassOf rdf:resource="&j2se-1_3;JavaSecurityAclAPI"/>
		<rdfs:comment xml:lang="en">JavaLibrary implementing the java.security.acl package for J2ME PP 1.1</rdfs:comment>
		<rdfs:comment xml:lang="OWLManchester">platform:comprisesInterfacePart some JavaSecurityAcl</rdfs:comment>
	</owl:Class>
	<owl:Class rdf:about="&j2me-pp-1_1;JavaNetAPI">
		<rdfs:subClassOf rdf:resource="&j2me-pp-1_0;JavaNetAPI"/>
		<rdfs:comment xml:lang="en">JavaLibrary implementing the java.net package for J2ME PP 1.1</rdfs:comment>
		<rdfs:comment xml:lang="OWLManchester">platform:comprisesInterfacePart some JavaNet</rdfs:comment>
	</owl:Class>
	<owl:Class rdf:about="&j2me-pp-1_1;JavaUtilAPI">
		<rdfs:subClassOf rdf:resource="&j2me-pp-1_0;JavaUtilAPI"/>
		<rdfs:comment xml:lang="en">JavaLibrary implementing the java.util package for J2ME PP 1.1</rdfs:comment>
		<rdfs:comment xml:lang="OWLManchester">platform:comprisesInterfacePart some JavaUtil</rdfs:comment>
	</owl:Class>
	<owl:Class rdf:about="&j2me-pp-1_1;JavaUtilJarAPI">
		<rdfs:subClassOf rdf:resource="&j2me-pp-1_0;JavaUtilJarAPI"/>
		<rdfs:subClassOf rdf:resource="&j2se-1_3;JavaUtilJarAPI"/>
		<rdfs:comment xml:lang="en">JavaLibrary implementing the java.util.jar package for J2ME PP 1.1</rdfs:comment>
		<rdfs:comment xml:lang="OWLManchester">platform:comprisesInterfacePart some JavaUtilJar</rdfs:comment>
	</owl:Class>
	<owl:Class rdf:about="&j2me-pp-1_1;JavaUtilZipAPI">
		<rdfs:subClassOf rdf:resource="&j2me-pp-1_0;JavaUtilZipAPI"/>
		<rdfs:subClassOf rdf:resource="&j2se-1_3;JavaUtilZipAPI"/>
		<rdfs:comment xml:lang="en">JavaLibrary implementing the java.util.zip package for J2ME PP 1.1</rdfs:comment>
		<rdfs:comment xml:lang="OWLManchester">platform:comprisesInterfacePart some JavaUtilZip</rdfs:comment>
	</owl:Class>
	<owl:Class rdf:about="&j2me-pp-1_1;JavaMathAPI">
		<owl:equivalentClass rdf:resource="&j2me-pp-1_0;JavaMathAPI"/>
		<owl:equivalentClass rdf:resource="&j2se-1_3;JavaMathAPI"/>
		<rdfs:subClassOf rdf:resource="&java;JavaAPI"/>
		<rdfs:comment xml:lang="en">JavaLibrary implementing the java.math package for J2ME PP 1.1</rdfs:comment>
		<rdfs:comment xml:lang="OWLManchester">platform:comprisesInterfacePart some JavaMath</rdfs:comment>
	</owl:Class>
	<owl:Class rdf:about="&j2me-pp-1_1;JavaTextAPI">
		<rdfs:subClassOf rdf:resource="&j2me-pp-1_0;JavaTextAPI"/>
		<rdfs:subClassOf rdf:resource="&j2se-1_3;JavaTextAPI"/>
		<rdfs:comment xml:lang="en">JavaLibrary implementing the java.text package for J2ME PP 1.1</rdfs:comment>
		<rdfs:comment xml:lang="OWLManchester">platform:comprisesInterfacePart some JavaText</rdfs:comment>
	</owl:Class>
	<owl:Class rdf:about="&j2me-pp-1_1;JavaAwtAPI">
		<rdfs:subClassOf rdf:resource="&j2me-pp-1_0;JavaAwtAPI"/>
		<rdfs:comment xml:lang="en">JavaLibrary implementing the java.awt package for J2ME PP 1.1</rdfs:comment>
		<rdfs:comment xml:lang="OWLManchester">platform:comprisesInterfacePart some JavaAwt</rdfs:comment>
	</owl:Class>
	<owl:Class rdf:about="&j2me-pp-1_1;JavaAwtImAPI">
		<rdfs:subClassOf rdf:resource="&java;JavaAPI"/>
		<rdfs:comment xml:lang="en">JavaLibrary implementing the java.awt.im package for J2ME PP 1.1</rdfs:comment>
		<rdfs:comment xml:lang="OWLManchester">platform:comprisesInterfacePart some JavaAwtIm</rdfs:comment>
	</owl:Class>
	<owl:Class rdf:about="&j2me-pp-1_1;JavaAwtFontAPI">
		<rdfs:subClassOf rdf:resource="&java;JavaAPI"/>
		<rdfs:comment xml:lang="en">JavaLibrary implementing the java.awt.font package for J2ME PP 1.1</rdfs:comment>
		<rdfs:comment xml:lang="OWLManchester">platform:comprisesInterfacePart some JavaAwtFont</rdfs:comment>
	</owl:Class>
	<owl:Class rdf:about="&j2me-pp-1_1;JavaAwtEventAPI">
		<rdfs:subClassOf rdf:resource="&j2me-pp-1_0;JavaAwtEventAPI"/>
		<rdfs:comment xml:lang="en">JavaLibrary implementing the java.awt.event package for J2ME PP 1.1</rdfs:comment>
		<rdfs:comment xml:lang="OWLManchester">platform:comprisesInterfacePart some JavaAwtEvent</rdfs:comment>
	</owl:Class>
	<owl:Class rdf:about="&j2me-pp-1_1;JavaAwtImageAPI">
		<rdfs:subClassOf rdf:resource="&j2me-pp-1_0;JavaAwtImageAPI"/>
		<rdfs:comment xml:lang="en">JavaLibrary implementing the java.awt.image package for J2ME PP 1.1</rdfs:comment>
		<rdfs:comment xml:lang="OWLManchester">platform:comprisesInterfacePart some JavaAwtImage</rdfs:comment>
	</owl:Class>
	<owl:Class rdf:about="&j2me-pp-1_1;JavaAwtColorAPI">
		<owl:equivalentClass rdf:resource="&j2me-pp-1_0;JavaAwtColorAPI"/>
		<rdfs:subClassOf rdf:resource="&java;JavaAPI"/>
		<rdfs:comment xml:lang="en">JavaLibrary implementing the java.awt.color package for J2ME PP 1.1</rdfs:comment>
		<rdfs:comment xml:lang="OWLManchester">platform:comprisesInterfacePart some JavaAwtColor</rdfs:comment>
	</owl:Class>
	<owl:Class rdf:about="&j2me-pp-1_1;JavaAwtDatatransferAPI">
		<rdfs:subClassOf rdf:resource="&j2me-pp-1_0;JavaAwtDatatransferAPI"/>
		<rdfs:comment xml:lang="en">JavaLibrary implementing the java.awt.datatransfer package for J2ME PP 1.1</rdfs:comment>
		<rdfs:comment xml:lang="OWLManchester">platform:comprisesInterfacePart some JavaAwtDatatransfer</rdfs:comment>
	</owl:Class>
	<owl:Class rdf:about="&j2me-pp-1_1;JavaBeansAPI">
		<rdfs:subClassOf rdf:resource="&j2me-pp-1_0;JavaBeansAPI"/>
		<rdfs:comment xml:lang="en">JavaLibrary implementing the java.beans package for J2ME PP 1.1</rdfs:comment>
		<rdfs:comment xml:lang="OWLManchester">platform:comprisesInterfacePart some JavaBeans</rdfs:comment>
	</owl:Class>
	<owl:Class rdf:about="&j2me-pp-1_1;JavaRmiAPI">
		<rdfs:subClassOf rdf:resource="&j2me-pp-1_0;JavaRmiAPI"/>
		<rdfs:comment xml:lang="en">JavaLibrary implementing the java.rmi package for J2ME PP 1.1</rdfs:comment>
		<rdfs:comment xml:lang="OWLManchester">platform:comprisesInterfacePart some JavaRmi</rdfs:comment>
	</owl:Class>
	<owl:Class rdf:about="&j2me-pp-1_1;JavaRmiRegistryAPI">
		<owl:equivalentClass rdf:resource="&j2me-pp-1_0;JavaRmiRegistryAPI"/>
		<rdfs:subClassOf rdf:resource="&java;JavaAPI"/>
		<rdfs:comment xml:lang="en">JavaLibrary implementing the java.rmi.registry package for J2ME PP 1.1</rdfs:comment>
		<rdfs:comment xml:lang="OWLManchester">platform:comprisesInterfacePart some JavaRmiRegistry</rdfs:comment>
	</owl:Class>
	<owl:Class rdf:about="&j2me-pp-1_1;JavaAppletAPI">
		<rdfs:subClassOf rdf:resource="&j2me-pp-1_0;JavaAppletAPI"/>
		<rdfs:comment xml:lang="en">JavaLibrary implementing the java.applet package for J2ME PP 1.1</rdfs:comment>
		<rdfs:comment xml:lang="OWLManchester">platform:comprisesInterfacePart some JavaApplet</rdfs:comment>
	</owl:Class>
	<owl:Class rdf:about="&j2me-pp-1_1;JavaxSecurityAuthX500API">
		<rdfs:subClassOf rdf:resource="&java;JavaAPI"/>
		<rdfs:comment xml:lang="en">JavaLibrary implementing the javax.security.auth.x500 package for J2ME PP 1.1</rdfs:comment>
		<rdfs:comment xml:lang="OWLManchester">platform:comprisesInterfacePart some JavaxSecurityAuthX500</rdfs:comment>
	</owl:Class>
	<owl:Class rdf:about="&j2me-pp-1_1;JavaxMicroeditionIoAPI">
		<rdfs:subClassOf rdf:resource="&j2me-pp-1_0;JavaxMicroeditionIoAPI"/>
		<rdfs:comment xml:lang="en">JavaLibrary implementing the javax.microedition.io package for J2ME PP 1.1</rdfs:comment>
		<rdfs:comment xml:lang="OWLManchester">platform:comprisesInterfacePart some JavaxMicroeditionIo</rdfs:comment>
	</owl:Class>
	<owl:Class rdf:about="&j2me-pp-1_1;JavaxMicroeditionPkiAPI">
		<rdfs:subClassOf rdf:resource="&java;JavaAPI"/>
		<rdfs:comment xml:lang="en">JavaLibrary implementing the javax.microedition.pki package for J2ME PP 1.1</rdfs:comment>
		<rdfs:comment xml:lang="OWLManchester">platform:comprisesInterfacePart some JavaxMicroeditionPki</rdfs:comment>
	</owl:Class>
	<owl:Class rdf:about="&j2me-pp-1_1;JavaxMicroeditionXletAPI">
		<rdfs:subClassOf rdf:resource="&j2me-pp-1_0;JavaxMicroeditionXletAPI"/>
		<rdfs:comment xml:lang="en">JavaLibrary implementing the javax.microedition.xlet package for J2ME PP 1.1</rdfs:comment>
		<rdfs:comment xml:lang="OWLManchester">platform:comprisesInterfacePart some JavaxMicroeditionXlet</rdfs:comment>
	</owl:Class>
	<owl:Class rdf:about="&j2me-pp-1_1;JavaxMicroeditionXletIxcAPI">
		<rdfs:subClassOf rdf:resource="&j2me-pp-1_0;JavaxMicroeditionXletIxcAPI"/>
		<rdfs:comment xml:lang="en">JavaLibrary implementing the javax.microedition.xlet.ixc package for J2ME PP 1.1</rdfs:comment>
		<rdfs:comment xml:lang="OWLManchester">platform:comprisesInterfacePart some JavaxMicroeditionXletIxc</rdfs:comment>
	</owl:Class>
	<j2me-pp-1_1:JavaIo rdf:about="&j2me-pp-1_1;theJavaIoPart">
	</j2me-pp-1_1:JavaIo>
	<j2me-pp-1_1:JavaLang rdf:about="&j2me-pp-1_1;theJavaLangPart">
	</j2me-pp-1_1:JavaLang>
	<j2me-pp-1_1:JavaLangRef rdf:about="&j2me-pp-1_1;theJavaLangRefPart">
	</j2me-pp-1_1:JavaLangRef>
	<j2me-pp-1_1:JavaLangReflect rdf:about="&j2me-pp-1_1;theJavaLangReflectPart">
	</j2me-pp-1_1:JavaLangReflect>
	<j2me-pp-1_1:JavaSecurity rdf:about="&j2me-pp-1_1;theJavaSecurityPart">
	</j2me-pp-1_1:JavaSecurity>
	<j2me-pp-1_1:JavaSecurityCert rdf:about="&j2me-pp-1_1;theJavaSecurityCertPart">
	</j2me-pp-1_1:JavaSecurityCert>
	<j2me-pp-1_1:JavaSecurityInterfaces rdf:about="&j2me-pp-1_1;theJavaSecurityInterfacesPart">
	</j2me-pp-1_1:JavaSecurityInterfaces>
	<j2me-pp-1_1:JavaSecuritySpec rdf:about="&j2me-pp-1_1;theJavaSecuritySpecPart">
	</j2me-pp-1_1:JavaSecuritySpec>
	<j2me-pp-1_1:JavaSecurityAcl rdf:about="&j2me-pp-1_1;theJavaSecurityAclPart">
	</j2me-pp-1_1:JavaSecurityAcl>
	<j2me-pp-1_1:JavaNet rdf:about="&j2me-pp-1_1;theJavaNetPart">
	</j2me-pp-1_1:JavaNet>
	<j2me-pp-1_1:JavaUtil rdf:about="&j2me-pp-1_1;theJavaUtilPart">
	</j2me-pp-1_1:JavaUtil>
	<j2me-pp-1_1:JavaUtilJar rdf:about="&j2me-pp-1_1;theJavaUtilJarPart">
	</j2me-pp-1_1:JavaUtilJar>
	<j2me-pp-1_1:JavaUtilZip rdf:about="&j2me-pp-1_1;theJavaUtilZipPart">
	</j2me-pp-1_1:JavaUtilZip>
	<j2me-pp-1_1:JavaMath rdf:about="&j2me-pp-1_1;theJavaMathPart">
	</j2me-pp-1_1:JavaMath>
	<j2me-pp-1_1:JavaText rdf:about="&j2me-pp-1_1;theJavaTextPart">
	</j2me-pp-1_1:JavaText>
	<j2me-pp-1_1:JavaAwt rdf:about="&j2me-pp-1_1;theJavaAwtPart">
	</j2me-pp-1_1:JavaAwt>
	<j2me-pp-1_1:JavaAwtIm rdf:about="&j2me-pp-1_1;theJavaAwtImPart">
	</j2me-pp-1_1:JavaAwtIm>
	<j2me-pp-1_1:JavaAwtFont rdf:about="&j2me-pp-1_1;theJavaAwtFontPart">
	</j2me-pp-1_1:JavaAwtFont>
	<j2me-pp-1_1:JavaAwtEvent rdf:about="&j2me-pp-1_1;theJavaAwtEventPart">
	</j2me-pp-1_1:JavaAwtEvent>
	<j2me-pp-1_1:JavaAwtImage rdf:about="&j2me-pp-1_1;theJavaAwtImagePart">
	</j2me-pp-1_1:JavaAwtImage>
	<j2me-pp-1_1:JavaAwtColor rdf:about="&j2me-pp-1_1;theJavaAwtColorPart">
	</j2me-pp-1_1:JavaAwtColor>
	<j2me-pp-1_1:JavaAwtDatatransfer rdf:about="&j2me-pp-1_1;theJavaAwtDatatransferPart">
	</j2me-pp-1_1:JavaAwtDatatransfer>
	<j2me-pp-1_1:JavaBeans rdf:about="&j2me-pp-1_1;theJavaBeansPart">
	</j2me-pp-1_1:JavaBeans>
	<j2me-pp-1_1:JavaRmi rdf:about="&j2me-pp-1_1;theJavaRmiPart">
	</j2me-pp-1_1:JavaRmi>
	<j2me-pp-1_1:JavaRmiRegistry rdf:about="&j2me-pp-1_1;theJavaRmiRegistryPart">
	</j2me-pp-1_1:JavaRmiRegistry>
	<j2me-pp-1_1:JavaApplet rdf:about="&j2me-pp-1_1;theJavaAppletPart">
	</j2me-pp-1_1:JavaApplet>
	<j2me-pp-1_1:JavaxSecurityAuthX500 rdf:about="&j2me-pp-1_1;theJavaxSecurityAuthX500Part">
	</j2me-pp-1_1:JavaxSecurityAuthX500>
	<j2me-pp-1_1:JavaxMicroeditionIo rdf:about="&j2me-pp-1_1;theJavaxMicroeditionIoPart">
	</j2me-pp-1_1:JavaxMicroeditionIo>
	<j2me-pp-1_1:JavaxMicroeditionPki rdf:about="&j2me-pp-1_1;theJavaxMicroeditionPkiPart">
	</j2me-pp-1_1:JavaxMicroeditionPki>
	<j2me-pp-1_1:JavaxMicroeditionXlet rdf:about="&j2me-pp-1_1;theJavaxMicroeditionXletPart">
	</j2me-pp-1_1:JavaxMicroeditionXlet>
	<j2me-pp-1_1:JavaxMicroeditionXletIxc rdf:about="&j2me-pp-1_1;theJavaxMicroeditionXletIxcPart">
	</j2me-pp-1_1:JavaxMicroeditionXletIxc>
	<owl:Class rdf:about="&j2me-pp-1_1;JavaIoClassLibrary">
		<rdfs:subClassOf rdf:resource="&j2me-pp-1_0;JavaIoClassLibrary"/>
		<rdfs:comment xml:lang="en">JavaLibrary implementing the java.io package for J2ME PP 1.1</rdfs:comment>
		<rdfs:comment xml:lang="OWLManchester">platform:implementsInterface some JavaIoAPI</rdfs:comment>
	</owl:Class>
	<owl:Class rdf:about="&j2me-pp-1_1;JavaLangClassLibrary">
		<rdfs:subClassOf rdf:resource="&j2me-pp-1_0;JavaLangClassLibrary"/>
		<rdfs:comment xml:lang="en">JavaLibrary implementing the java.lang package for J2ME PP 1.1</rdfs:comment>
		<rdfs:comment xml:lang="OWLManchester">platform:implementsInterface some JavaLangAPI</rdfs:comment>
	</owl:Class>
	<owl:Class rdf:about="&j2me-pp-1_1;JavaLangRefClassLibrary">
		<owl:equivalentClass rdf:resource="&j2me-pp-1_0;JavaLangRefClassLibrary"/>
		<owl:equivalentClass rdf:resource="&j2se-1_3;JavaLangRefClassLibrary"/>
		<rdfs:subClassOf rdf:resource="&java;JavaClassLibrary"/>
		<rdfs:comment xml:lang="en">JavaLibrary implementing the java.lang.ref package for J2ME PP 1.1</rdfs:comment>
		<rdfs:comment xml:lang="OWLManchester">platform:implementsInterface some JavaLangRefAPI</rdfs:comment>
	</owl:Class>
	<owl:Class rdf:about="&j2me-pp-1_1;JavaLangReflectClassLibrary">
		<rdfs:subClassOf rdf:resource="&j2me-pp-1_0;JavaLangReflectClassLibrary"/>
		<rdfs:subClassOf rdf:resource="&j2se-1_3;JavaLangReflectClassLibrary"/>
		<rdfs:comment xml:lang="en">JavaLibrary implementing the java.lang.reflect package for J2ME PP 1.1</rdfs:comment>
		<rdfs:comment xml:lang="OWLManchester">platform:implementsInterface some JavaLangReflectAPI</rdfs:comment>
	</owl:Class>
	<owl:Class rdf:about="&j2me-pp-1_1;JavaSecurityClassLibrary">
		<rdfs:subClassOf rdf:resource="&j2me-pp-1_0;JavaSecurityClassLibrary"/>
		<rdfs:comment xml:lang="en">JavaLibrary implementing the java.security package for J2ME PP 1.1</rdfs:comment>
		<rdfs:comment xml:lang="OWLManchester">platform:implementsInterface some JavaSecurityAPI</rdfs:comment>
	</owl:Class>
	<owl:Class rdf:about="&j2me-pp-1_1;JavaSecurityCertClassLibrary">
		<rdfs:subClassOf rdf:resource="&j2me-pp-1_0;JavaSecurityCertClassLibrary"/>
		<rdfs:subClassOf rdf:resource="&j2se-1_3;JavaSecurityCertClassLibrary"/>
		<rdfs:comment xml:lang="en">JavaLibrary implementing the java.security.cert package for J2ME PP 1.1</rdfs:comment>
		<rdfs:comment xml:lang="OWLManchester">platform:implementsInterface some JavaSecurityCertAPI</rdfs:comment>
	</owl:Class>
	<owl:Class rdf:about="&j2me-pp-1_1;JavaSecurityInterfacesClassLibrary">
		<owl:equivalentClass rdf:resource="&j2me-pp-1_0;JavaSecurityInterfacesClassLibrary"/>
		<owl:equivalentClass rdf:resource="&j2se-1_3;JavaSecurityInterfacesClassLibrary"/>
		<rdfs:subClassOf rdf:resource="&java;JavaClassLibrary"/>
		<rdfs:comment xml:lang="en">JavaLibrary implementing the java.security.interfaces package for J2ME PP 1.1</rdfs:comment>
		<rdfs:comment xml:lang="OWLManchester">platform:implementsInterface some JavaSecurityInterfacesAPI</rdfs:comment>
	</owl:Class>
	<owl:Class rdf:about="&j2me-pp-1_1;JavaSecuritySpecClassLibrary">
		<rdfs:subClassOf rdf:resource="&j2me-pp-1_0;JavaSecuritySpecClassLibrary"/>
		<rdfs:subClassOf rdf:resource="&j2se-1_3;JavaSecuritySpecClassLibrary"/>
		<rdfs:comment xml:lang="en">JavaLibrary implementing the java.security.spec package for J2ME PP 1.1</rdfs:comment>
		<rdfs:comment xml:lang="OWLManchester">platform:implementsInterface some JavaSecuritySpecAPI</rdfs:comment>
	</owl:Class>
	<owl:Class rdf:about="&j2me-pp-1_1;JavaSecurityAclClassLibrary">
		<rdfs:subClassOf rdf:resource="&j2me-pp-1_0;JavaSecurityAclClassLibrary"/>
		<rdfs:subClassOf rdf:resource="&j2se-1_3;JavaSecurityAclClassLibrary"/>
		<rdfs:comment xml:lang="en">JavaLibrary implementing the java.security.acl package for J2ME PP 1.1</rdfs:comment>
		<rdfs:comment xml:lang="OWLManchester">platform:implementsInterface some JavaSecurityAclAPI</rdfs:comment>
	</owl:Class>
	<owl:Class rdf:about="&j2me-pp-1_1;JavaNetClassLibrary">
		<rdfs:subClassOf rdf:resource="&j2me-pp-1_0;JavaNetClassLibrary"/>
		<rdfs:comment xml:lang="en">JavaLibrary implementing the java.net package for J2ME PP 1.1</rdfs:comment>
		<rdfs:comment xml:lang="OWLManchester">platform:implementsInterface some JavaNetAPI</rdfs:comment>
	</owl:Class>
	<owl:Class rdf:about="&j2me-pp-1_1;JavaUtilClassLibrary">
		<rdfs:subClassOf rdf:resource="&j2me-pp-1_0;JavaUtilClassLibrary"/>
		<rdfs:comment xml:lang="en">JavaLibrary implementing the java.util package for J2ME PP 1.1</rdfs:comment>
		<rdfs:comment xml:lang="OWLManchester">platform:implementsInterface some JavaUtilAPI</rdfs:comment>
	</owl:Class>
	<owl:Class rdf:about="&j2me-pp-1_1;JavaUtilJarClassLibrary">
		<rdfs:subClassOf rdf:resource="&j2me-pp-1_0;JavaUtilJarClassLibrary"/>
		<rdfs:subClassOf rdf:resource="&j2se-1_3;JavaUtilJarClassLibrary"/>
		<rdfs:comment xml:lang="en">JavaLibrary implementing the java.util.jar package for J2ME PP 1.1</rdfs:comment>
		<rdfs:comment xml:lang="OWLManchester">platform:implementsInterface some JavaUtilJarAPI</rdfs:comment>
	</owl:Class>
	<owl:Class rdf:about="&j2me-pp-1_1;JavaUtilZipClassLibrary">
		<rdfs:subClassOf rdf:resource="&j2me-pp-1_0;JavaUtilZipClassLibrary"/>
		<rdfs:subClassOf rdf:resource="&j2se-1_3;JavaUtilZipClassLibrary"/>
		<rdfs:comment xml:lang="en">JavaLibrary implementing the java.util.zip package for J2ME PP 1.1</rdfs:comment>
		<rdfs:comment xml:lang="OWLManchester">platform:implementsInterface some JavaUtilZipAPI</rdfs:comment>
	</owl:Class>
	<owl:Class rdf:about="&j2me-pp-1_1;JavaMathClassLibrary">
		<owl:equivalentClass rdf:resource="&j2me-pp-1_0;JavaMathClassLibrary"/>
		<owl:equivalentClass rdf:resource="&j2se-1_3;JavaMathClassLibrary"/>
		<rdfs:subClassOf rdf:resource="&java;JavaClassLibrary"/>
		<rdfs:comment xml:lang="en">JavaLibrary implementing the java.math package for J2ME PP 1.1</rdfs:comment>
		<rdfs:comment xml:lang="OWLManchester">platform:implementsInterface some JavaMathAPI</rdfs:comment>
	</owl:Class>
	<owl:Class rdf:about="&j2me-pp-1_1;JavaTextClassLibrary">
		<rdfs:subClassOf rdf:resource="&j2me-pp-1_0;JavaTextClassLibrary"/>
		<rdfs:subClassOf rdf:resource="&j2se-1_3;JavaTextClassLibrary"/>
		<rdfs:comment xml:lang="en">JavaLibrary implementing the java.text package for J2ME PP 1.1</rdfs:comment>
		<rdfs:comment xml:lang="OWLManchester">platform:implementsInterface some JavaTextAPI</rdfs:comment>
	</owl:Class>
	<owl:Class rdf:about="&j2me-pp-1_1;JavaAwtClassLibrary">
		<rdfs:subClassOf rdf:resource="&j2me-pp-1_0;JavaAwtClassLibrary"/>
		<rdfs:comment xml:lang="en">JavaLibrary implementing the java.awt package for J2ME PP 1.1</rdfs:comment>
		<rdfs:comment xml:lang="OWLManchester">platform:implementsInterface some JavaAwtAPI</rdfs:comment>
	</owl:Class>
	<owl:Class rdf:about="&j2me-pp-1_1;JavaAwtImClassLibrary">
		<rdfs:subClassOf rdf:resource="&java;JavaClassLibrary"/>
		<rdfs:comment xml:lang="en">JavaLibrary implementing the java.awt.im package for J2ME PP 1.1</rdfs:comment>
		<rdfs:comment xml:lang="OWLManchester">platform:implementsInterface some JavaAwtImAPI</rdfs:comment>
	</owl:Class>
	<owl:Class rdf:about="&j2me-pp-1_1;JavaAwtFontClassLibrary">
		<rdfs:subClassOf rdf:resource="&java;JavaClassLibrary"/>
		<rdfs:comment xml:lang="en">JavaLibrary implementing the java.awt.font package for J2ME PP 1.1</rdfs:comment>
		<rdfs:comment xml:lang="OWLManchester">platform:implementsInterface some JavaAwtFontAPI</rdfs:comment>
	</owl:Class>
	<owl:Class rdf:about="&j2me-pp-1_1;JavaAwtEventClassLibrary">
		<rdfs:subClassOf rdf:resource="&j2me-pp-1_0;JavaAwtEventClassLibrary"/>
		<rdfs:comment xml:lang="en">JavaLibrary implementing the java.awt.event package for J2ME PP 1.1</rdfs:comment>
		<rdfs:comment xml:lang="OWLManchester">platform:implementsInterface some JavaAwtEventAPI</rdfs:comment>
	</owl:Class>
	<owl:Class rdf:about="&j2me-pp-1_1;JavaAwtImageClassLibrary">
		<rdfs:subClassOf rdf:resource="&j2me-pp-1_0;JavaAwtImageClassLibrary"/>
		<rdfs:comment xml:lang="en">JavaLibrary implementing the java.awt.image package for J2ME PP 1.1</rdfs:comment>
		<rdfs:comment xml:lang="OWLManchester">platform:implementsInterface some JavaAwtImageAPI</rdfs:comment>
	</owl:Class>
	<owl:Class rdf:about="&j2me-pp-1_1;JavaAwtColorClassLibrary">
		<owl:equivalentClass rdf:resource="&j2me-pp-1_0;JavaAwtColorClassLibrary"/>
		<rdfs:subClassOf rdf:resource="&java;JavaClassLibrary"/>
		<rdfs:comment xml:lang="en">JavaLibrary implementing the java.awt.color package for J2ME PP 1.1</rdfs:comment>
		<rdfs:comment xml:lang="OWLManchester">platform:implementsInterface some JavaAwtColorAPI</rdfs:comment>
	</owl:Class>
	<owl:Class rdf:about="&j2me-pp-1_1;JavaAwtDatatransferClassLibrary">
		<rdfs:subClassOf rdf:resource="&j2me-pp-1_0;JavaAwtDatatransferClassLibrary"/>
		<rdfs:comment xml:lang="en">JavaLibrary implementing the java.awt.datatransfer package for J2ME PP 1.1</rdfs:comment>
		<rdfs:comment xml:lang="OWLManchester">platform:implementsInterface some JavaAwtDatatransferAPI</rdfs:comment>
	</owl:Class>
	<owl:Class rdf:about="&j2me-pp-1_1;JavaBeansClassLibrary">
		<rdfs:subClassOf rdf:resource="&j2me-pp-1_0;JavaBeansClassLibrary"/>
		<rdfs:comment xml:lang="en">JavaLibrary implementing the java.beans package for J2ME PP 1.1</rdfs:comment>
		<rdfs:comment xml:lang="OWLManchester">platform:implementsInterface some JavaBeansAPI</rdfs:comment>
	</owl:Class>
	<owl:Class rdf:about="&j2me-pp-1_1;JavaRmiClassLibrary">
		<rdfs:subClassOf rdf:resource="&j2me-pp-1_0;JavaRmiClassLibrary"/>
		<rdfs:comment xml:lang="en">JavaLibrary implementing the java.rmi package for J2ME PP 1.1</rdfs:comment>
		<rdfs:comment xml:lang="OWLManchester">platform:implementsInterface some JavaRmiAPI</rdfs:comment>
	</owl:Class>
	<owl:Class rdf:about="&j2me-pp-1_1;JavaRmiRegistryClassLibrary">
		<owl:equivalentClass rdf:resource="&j2me-pp-1_0;JavaRmiRegistryClassLibrary"/>
		<rdfs:subClassOf rdf:resource="&java;JavaClassLibrary"/>
		<rdfs:comment xml:lang="en">JavaLibrary implementing the java.rmi.registry package for J2ME PP 1.1</rdfs:comment>
		<rdfs:comment xml:lang="OWLManchester">platform:implementsInterface some JavaRmiRegistryAPI</rdfs:comment>
	</owl:Class>
	<owl:Class rdf:about="&j2me-pp-1_1;JavaAppletClassLibrary">
		<rdfs:subClassOf rdf:resource="&j2me-pp-1_0;JavaAppletClassLibrary"/>
		<rdfs:comment xml:lang="en">JavaLibrary implementing the java.applet package for J2ME PP 1.1</rdfs:comment>
		<rdfs:comment xml:lang="OWLManchester">platform:implementsInterface some JavaAppletAPI</rdfs:comment>
	</owl:Class>
	<owl:Class rdf:about="&j2me-pp-1_1;JavaxSecurityAuthX500ClassLibrary">
		<rdfs:subClassOf rdf:resource="&java;JavaClassLibrary"/>
		<rdfs:comment xml:lang="en">JavaLibrary implementing the javax.security.auth.x500 package for J2ME PP 1.1</rdfs:comment>
		<rdfs:comment xml:lang="OWLManchester">platform:implementsInterface some JavaxSecurityAuthX500API</rdfs:comment>
	</owl:Class>
	<owl:Class rdf:about="&j2me-pp-1_1;JavaxMicroeditionIoClassLibrary">
		<rdfs:subClassOf rdf:resource="&j2me-pp-1_0;JavaxMicroeditionIoClassLibrary"/>
		<rdfs:comment xml:lang="en">JavaLibrary implementing the javax.microedition.io package for J2ME PP 1.1</rdfs:comment>
		<rdfs:comment xml:lang="OWLManchester">platform:implementsInterface some JavaxMicroeditionIoAPI</rdfs:comment>
	</owl:Class>
	<owl:Class rdf:about="&j2me-pp-1_1;JavaxMicroeditionPkiClassLibrary">
		<rdfs:subClassOf rdf:resource="&java;JavaClassLibrary"/>
		<rdfs:comment xml:lang="en">JavaLibrary implementing the javax.microedition.pki package for J2ME PP 1.1</rdfs:comment>
		<rdfs:comment xml:lang="OWLManchester">platform:implementsInterface some JavaxMicroeditionPkiAPI</rdfs:comment>
	</owl:Class>
	<owl:Class rdf:about="&j2me-pp-1_1;JavaxMicroeditionXletClassLibrary">
		<rdfs:subClassOf rdf:resource="&j2me-pp-1_0;JavaxMicroeditionXletClassLibrary"/>
		<rdfs:comment xml:lang="en">JavaLibrary implementing the javax.microedition.xlet package for J2ME PP 1.1</rdfs:comment>
		<rdfs:comment xml:lang="OWLManchester">platform:implementsInterface some JavaxMicroeditionXletAPI</rdfs:comment>
	</owl:Class>
	<owl:Class rdf:about="&j2me-pp-1_1;JavaxMicroeditionXletIxcClassLibrary">
		<rdfs:subClassOf rdf:resource="&j2me-pp-1_0;JavaxMicroeditionXletIxcClassLibrary"/>
		<rdfs:comment xml:lang="en">JavaLibrary implementing the javax.microedition.xlet.ixc package for J2ME PP 1.1</rdfs:comment>
		<rdfs:comment xml:lang="OWLManchester">platform:implementsInterface some JavaxMicroeditionXletIxcAPI</rdfs:comment>
	</owl:Class>
</rdf:RDF>
