<?xml version="1.0" encoding="ISO-8859-1"?>
<!DOCTYPE rdf:RDF [
	<!ENTITY ns_19 "http://localhost/~dennis/platformkit/2010_1/">
	<!ENTITY platform "http://localhost/~dennis/platformkit/2010_1/platform.owl#">
	<!ENTITY xsd "http://www.w3.org/2001/XMLSchema#">
	<!ENTITY j2se-1_2 "http://soft.vub.ac.be/platformkit/2010/1/j2se-1_2.owl#">
	<!ENTITY isa "http://localhost/~dennis/platformkit/2010_1/isa.owl#">
	<!ENTITY j2me-midp-1_0 "http://soft.vub.ac.be/platformkit/2010/1/j2me-midp-1_0.owl#">
	<!ENTITY java "http://localhost/~dennis/platformkit/2010_1/java.owl#">
	<!ENTITY j2me-midp-2_0 "http://soft.vub.ac.be/platformkit/2010/1/j2me-midp-2_0.owl#">
	<!ENTITY j2me-pp-1_0 "http://soft.vub.ac.be/platformkit/2010/1/j2me-pp-1_0.owl#">
	<!ENTITY owl "http://www.w3.org/2002/07/owl#">
	<!ENTITY rdfs "http://www.w3.org/2000/01/rdf-schema#">
	<!ENTITY rdf "http://www.w3.org/1999/02/22-rdf-syntax-ns#">
]>
<rdf:RDF
	 xmlns:ns_19="&ns_19;"
	 xmlns:platform="&platform;"
	 xmlns:xsd="&xsd;"
	 xmlns:j2se-1_2="&j2se-1_2;"
	 xmlns:isa="&isa;"
	 xmlns:j2me-midp-1_0="&j2me-midp-1_0;"
	 xmlns:java="&java;"
	 xmlns:j2me-midp-2_0="&j2me-midp-2_0;"
	 xmlns:j2me-pp-1_0="&j2me-pp-1_0;"
	 xmlns:owl="&owl;"
	 xmlns:rdfs="&rdfs;"
	 xmlns:rdf="&rdf;"
>

	<owl:Ontology rdf:about="http://soft.vub.ac.be/platformkit/2010/1/j2me-pp-1_0.owl#">
		<owl:versionInfo>$Id: UML2ToPackageAPIOntology.atl 8082 2010-03-18 21:11:00Z dwagelaa $</owl:versionInfo>
		<owl:imports rdf:resource="http://localhost/~dennis/platformkit/2010_1/platform.owl"/>
		<owl:imports rdf:resource="http://localhost/~dennis/platformkit/2010_1/java.owl"/>
		<owl:imports rdf:resource="http://soft.vub.ac.be/platformkit/2010/1/j2me-midp-2_0.owl#"/>
		<owl:imports rdf:resource="http://soft.vub.ac.be/platformkit/2010/1/j2se-1_2.owl#"/>
		<owl:imports rdf:resource="http://soft.vub.ac.be/platformkit/2010/1/j2me-midp-1_0.owl#"/>
		<owl:imports rdf:resource="http://localhost/~dennis/platformkit/2010_1/isa.owl"/>
		<rdfs:comment xml:lang="en">Generated by [UML2ToSimplifiedPackageAPIOntology.atl 8080 2010-03-18 10:46:40Z dwagelaa], [UML2ToPackageAPIOntology.atl 8082 2010-03-18 21:11:00Z dwagelaa], [UML2ToAPIOntology.atl 8082 2010-03-18 21:11:00Z dwagelaa], and [UML2Comparison.atl 8082 2010-03-18 21:11:00Z dwagelaa]</rdfs:comment>
		<rdfs:comment>Dennis Wagelaar &lt;dennis.wagelaar@vub.ac.be&gt;</rdfs:comment>
		<rdfs:comment xml:lang="en">&#169; 2010, Vrije Universiteit Brussel. All rights reserved.</rdfs:comment>
		<rdfs:label xml:lang="en">J2ME PP 1.0</rdfs:label>
	</owl:Ontology>
	<owl:Class rdf:about="&j2me-pp-1_0;J2MEPP1_0API">
		<rdfs:subClassOf rdf:resource="&j2me-pp-1_0;JavaIoAPI"/>
		<rdfs:subClassOf rdf:resource="&j2me-pp-1_0;JavaLangAPI"/>
		<rdfs:subClassOf rdf:resource="&j2me-pp-1_0;JavaLangReflectAPI"/>
		<rdfs:subClassOf rdf:resource="&j2me-pp-1_0;JavaLangRefAPI"/>
		<rdfs:subClassOf rdf:resource="&j2me-pp-1_0;JavaNetAPI"/>
		<rdfs:subClassOf rdf:resource="&j2me-pp-1_0;JavaSecurityAPI"/>
		<rdfs:subClassOf rdf:resource="&j2me-pp-1_0;JavaSecurityCertAPI"/>
		<rdfs:subClassOf rdf:resource="&j2me-pp-1_0;JavaSecuritySpecAPI"/>
		<rdfs:subClassOf rdf:resource="&j2me-pp-1_0;JavaSecurityInterfacesAPI"/>
		<rdfs:subClassOf rdf:resource="&j2me-pp-1_0;JavaSecurityAclAPI"/>
		<rdfs:subClassOf rdf:resource="&j2me-pp-1_0;JavaUtilAPI"/>
		<rdfs:subClassOf rdf:resource="&j2me-pp-1_0;JavaUtilJarAPI"/>
		<rdfs:subClassOf rdf:resource="&j2me-pp-1_0;JavaUtilZipAPI"/>
		<rdfs:subClassOf rdf:resource="&j2me-pp-1_0;JavaMathAPI"/>
		<rdfs:subClassOf rdf:resource="&j2me-pp-1_0;JavaTextAPI"/>
		<rdfs:subClassOf rdf:resource="&j2me-pp-1_0;JavaTextResourcesAPI"/>
		<rdfs:subClassOf rdf:resource="&j2me-pp-1_0;JavaAppletAPI"/>
		<rdfs:subClassOf rdf:resource="&j2me-pp-1_0;JavaAwtAPI"/>
		<rdfs:subClassOf rdf:resource="&j2me-pp-1_0;JavaAwtEventAPI"/>
		<rdfs:subClassOf rdf:resource="&j2me-pp-1_0;JavaAwtImageAPI"/>
		<rdfs:subClassOf rdf:resource="&j2me-pp-1_0;JavaAwtColorAPI"/>
		<rdfs:subClassOf rdf:resource="&j2me-pp-1_0;JavaAwtDatatransferAPI"/>
		<rdfs:subClassOf rdf:resource="&j2me-pp-1_0;JavaBeansAPI"/>
		<rdfs:subClassOf rdf:resource="&j2me-pp-1_0;JavaRmiAPI"/>
		<rdfs:subClassOf rdf:resource="&j2me-pp-1_0;JavaRmiRegistryAPI"/>
		<rdfs:subClassOf rdf:resource="&j2me-pp-1_0;JavaxMicroeditionIoAPI"/>
		<rdfs:subClassOf rdf:resource="&j2me-pp-1_0;JavaxMicroeditionXletAPI"/>
		<rdfs:subClassOf rdf:resource="&j2me-pp-1_0;JavaxMicroeditionXletIxcAPI"/>
		<rdfs:comment xml:lang="en">J2ME PP 1.0 API</rdfs:comment>
		<rdfs:comment xml:lang="OWLManchester">platform:comprisesInterfacePart some JavaIo and platform:comprisesInterfacePart some JavaLang and platform:comprisesInterfacePart some JavaLangReflect and platform:comprisesInterfacePart some JavaLangRef and platform:comprisesInterfacePart some JavaNet and platform:comprisesInterfacePart some JavaSecurity and platform:comprisesInterfacePart some JavaSecurityCert and platform:comprisesInterfacePart some JavaSecuritySpec and platform:comprisesInterfacePart some JavaSecurityInterfaces and platform:comprisesInterfacePart some JavaSecurityAcl and platform:comprisesInterfacePart some JavaUtil and platform:comprisesInterfacePart some JavaUtilJar and platform:comprisesInterfacePart some JavaUtilZip and platform:comprisesInterfacePart some JavaMath and platform:comprisesInterfacePart some JavaText and platform:comprisesInterfacePart some JavaTextResources and platform:comprisesInterfacePart some JavaApplet and platform:comprisesInterfacePart some JavaAwt and platform:comprisesInterfacePart some JavaAwtEvent and platform:comprisesInterfacePart some JavaAwtImage and platform:comprisesInterfacePart some JavaAwtColor and platform:comprisesInterfacePart some JavaAwtDatatransfer and platform:comprisesInterfacePart some JavaBeans and platform:comprisesInterfacePart some JavaRmi and platform:comprisesInterfacePart some JavaRmiRegistry and platform:comprisesInterfacePart some JavaxMicroeditionIo and platform:comprisesInterfacePart some JavaxMicroeditionXlet and platform:comprisesInterfacePart some JavaxMicroeditionXletIxc</rdfs:comment>
	</owl:Class>
	<owl:Class rdf:about="&j2me-pp-1_0;J2MEPP1_0ClassLibrary">
		<rdfs:subClassOf rdf:resource="&j2me-pp-1_0;JavaIoClassLibrary"/>
		<rdfs:subClassOf rdf:resource="&j2me-pp-1_0;JavaLangClassLibrary"/>
		<rdfs:subClassOf rdf:resource="&j2me-pp-1_0;JavaLangReflectClassLibrary"/>
		<rdfs:subClassOf rdf:resource="&j2me-pp-1_0;JavaLangRefClassLibrary"/>
		<rdfs:subClassOf rdf:resource="&j2me-pp-1_0;JavaNetClassLibrary"/>
		<rdfs:subClassOf rdf:resource="&j2me-pp-1_0;JavaSecurityClassLibrary"/>
		<rdfs:subClassOf rdf:resource="&j2me-pp-1_0;JavaSecurityCertClassLibrary"/>
		<rdfs:subClassOf rdf:resource="&j2me-pp-1_0;JavaSecuritySpecClassLibrary"/>
		<rdfs:subClassOf rdf:resource="&j2me-pp-1_0;JavaSecurityInterfacesClassLibrary"/>
		<rdfs:subClassOf rdf:resource="&j2me-pp-1_0;JavaSecurityAclClassLibrary"/>
		<rdfs:subClassOf rdf:resource="&j2me-pp-1_0;JavaUtilClassLibrary"/>
		<rdfs:subClassOf rdf:resource="&j2me-pp-1_0;JavaUtilJarClassLibrary"/>
		<rdfs:subClassOf rdf:resource="&j2me-pp-1_0;JavaUtilZipClassLibrary"/>
		<rdfs:subClassOf rdf:resource="&j2me-pp-1_0;JavaMathClassLibrary"/>
		<rdfs:subClassOf rdf:resource="&j2me-pp-1_0;JavaTextClassLibrary"/>
		<rdfs:subClassOf rdf:resource="&j2me-pp-1_0;JavaTextResourcesClassLibrary"/>
		<rdfs:subClassOf rdf:resource="&j2me-pp-1_0;JavaAppletClassLibrary"/>
		<rdfs:subClassOf rdf:resource="&j2me-pp-1_0;JavaAwtClassLibrary"/>
		<rdfs:subClassOf rdf:resource="&j2me-pp-1_0;JavaAwtEventClassLibrary"/>
		<rdfs:subClassOf rdf:resource="&j2me-pp-1_0;JavaAwtImageClassLibrary"/>
		<rdfs:subClassOf rdf:resource="&j2me-pp-1_0;JavaAwtColorClassLibrary"/>
		<rdfs:subClassOf rdf:resource="&j2me-pp-1_0;JavaAwtDatatransferClassLibrary"/>
		<rdfs:subClassOf rdf:resource="&j2me-pp-1_0;JavaBeansClassLibrary"/>
		<rdfs:subClassOf rdf:resource="&j2me-pp-1_0;JavaRmiClassLibrary"/>
		<rdfs:subClassOf rdf:resource="&j2me-pp-1_0;JavaRmiRegistryClassLibrary"/>
		<rdfs:subClassOf rdf:resource="&j2me-pp-1_0;JavaxMicroeditionIoClassLibrary"/>
		<rdfs:subClassOf rdf:resource="&j2me-pp-1_0;JavaxMicroeditionXletClassLibrary"/>
		<rdfs:subClassOf rdf:resource="&j2me-pp-1_0;JavaxMicroeditionXletIxcClassLibrary"/>
		<rdfs:comment xml:lang="en">Java class library implementing the J2ME PP 1.0 API</rdfs:comment>
		<rdfs:comment xml:lang="OWLManchester">platform:implementsInterface some J2MEPP1_0API</rdfs:comment>
	</owl:Class>
	<owl:Class rdf:about="&j2me-pp-1_0;J2MEPP1_0BytecodeFormat">
		<rdfs:subClassOf rdf:resource="&j2se-1_2;J2SE1_2BytecodeFormat"/>
		<rdfs:subClassOf rdf:resource="&j2me-midp-2_0;J2MEMIDP2_0BytecodeFormat"/>
		<rdfs:subClassOf rdf:resource="&j2me-midp-1_0;J2MEMIDP1_0BytecodeFormat"/>
		<rdfs:comment xml:lang="en">J2ME PP 1.0 bytecode format</rdfs:comment>
		<rdfs:comment xml:lang="OWLManchester">java:majorVersionNumber some xsd:integer[>="47"^^xsd:integer] and java:preverified value false</rdfs:comment>
	</owl:Class>
	<j2me-pp-1_0:J2MEPP1_0BytecodeFormat rdf:about="&j2me-pp-1_0;theJ2MEPP1_0BytecodeFormat">
		<java:preverified rdf:datatype="http://www.w3.org/2001/XMLSchema#boolean">false</java:preverified>
		<java:minorVersionNumber rdf:datatype="http://www.w3.org/2001/XMLSchema#integer">0</java:minorVersionNumber>
		<java:majorVersionNumber rdf:datatype="http://www.w3.org/2001/XMLSchema#integer">47</java:majorVersionNumber>
	</j2me-pp-1_0:J2MEPP1_0BytecodeFormat>
	<j2me-pp-1_0:J2MEPP1_0API rdf:about="&j2me-pp-1_0;theJ2MEPP1_0API">
		<platform:comprisesInterfacePart rdf:resource="&j2me-pp-1_0;theJavaxMicroeditionXletIxcPart"/>
		<platform:comprisesInterfacePart rdf:resource="&j2me-pp-1_0;theJavaxMicroeditionXletPart"/>
		<platform:comprisesInterfacePart rdf:resource="&j2me-pp-1_0;theJavaxMicroeditionIoPart"/>
		<platform:comprisesInterfacePart rdf:resource="&j2me-pp-1_0;theJavaRmiRegistryPart"/>
		<platform:comprisesInterfacePart rdf:resource="&j2me-pp-1_0;theJavaRmiPart"/>
		<platform:comprisesInterfacePart rdf:resource="&j2me-pp-1_0;theJavaBeansPart"/>
		<platform:comprisesInterfacePart rdf:resource="&j2me-pp-1_0;theJavaAwtDatatransferPart"/>
		<platform:comprisesInterfacePart rdf:resource="&j2me-pp-1_0;theJavaAwtColorPart"/>
		<platform:comprisesInterfacePart rdf:resource="&j2me-pp-1_0;theJavaAwtImagePart"/>
		<platform:comprisesInterfacePart rdf:resource="&j2me-pp-1_0;theJavaAwtEventPart"/>
		<platform:comprisesInterfacePart rdf:resource="&j2me-pp-1_0;theJavaAwtPart"/>
		<platform:comprisesInterfacePart rdf:resource="&j2me-pp-1_0;theJavaAppletPart"/>
		<platform:comprisesInterfacePart rdf:resource="&j2me-pp-1_0;theJavaTextResourcesPart"/>
		<platform:comprisesInterfacePart rdf:resource="&j2me-pp-1_0;theJavaTextPart"/>
		<platform:comprisesInterfacePart rdf:resource="&j2me-pp-1_0;theJavaMathPart"/>
		<platform:comprisesInterfacePart rdf:resource="&j2me-pp-1_0;theJavaUtilZipPart"/>
		<platform:comprisesInterfacePart rdf:resource="&j2me-pp-1_0;theJavaUtilJarPart"/>
		<platform:comprisesInterfacePart rdf:resource="&j2me-pp-1_0;theJavaUtilPart"/>
		<platform:comprisesInterfacePart rdf:resource="&j2me-pp-1_0;theJavaSecurityAclPart"/>
		<platform:comprisesInterfacePart rdf:resource="&j2me-pp-1_0;theJavaSecurityInterfacesPart"/>
		<platform:comprisesInterfacePart rdf:resource="&j2me-pp-1_0;theJavaSecuritySpecPart"/>
		<platform:comprisesInterfacePart rdf:resource="&j2me-pp-1_0;theJavaSecurityCertPart"/>
		<platform:comprisesInterfacePart rdf:resource="&j2me-pp-1_0;theJavaSecurityPart"/>
		<platform:comprisesInterfacePart rdf:resource="&j2me-pp-1_0;theJavaNetPart"/>
		<platform:comprisesInterfacePart rdf:resource="&j2me-pp-1_0;theJavaLangRefPart"/>
		<platform:comprisesInterfacePart rdf:resource="&j2me-pp-1_0;theJavaLangReflectPart"/>
		<platform:comprisesInterfacePart rdf:resource="&j2me-pp-1_0;theJavaLangPart"/>
		<platform:comprisesInterfacePart rdf:resource="&j2me-pp-1_0;theJavaIoPart"/>
	</j2me-pp-1_0:J2MEPP1_0API>
	<owl:Class rdf:about="&j2me-pp-1_0;J2MEPP1_0VM">
		<owl:equivalentClass>
			<owl:Restriction>
				<owl:onProperty rdf:resource="&platform;implementsInterface"/>
				<owl:someValuesFrom rdf:resource="&j2me-pp-1_0;J2MEPP1_0BytecodeFormat"/>
			</owl:Restriction>
		</owl:equivalentClass>
		<rdfs:subClassOf rdf:resource="&java;JavaVM"/>
		<rdfs:comment xml:lang="en">J2ME PP 1.0 virtual machine</rdfs:comment>
	</owl:Class>
	<owl:Class rdf:about="&j2me-pp-1_0;J2MEPP1_0JRE">
		<owl:equivalentClass>
			<owl:Class >
				<owl:intersectionOf rdf:parseType="Collection">
					<owl:Restriction>
						<owl:onProperty rdf:resource="&platform;providesFeature"/>
						<owl:someValuesFrom rdf:resource="&j2me-pp-1_0;J2MEPP1_0ClassLibrary"/>
					</owl:Restriction>
					<owl:Restriction>
						<owl:onProperty rdf:resource="&platform;providesFeature"/>
						<owl:someValuesFrom rdf:resource="&j2me-pp-1_0;J2MEPP1_0VM"/>
					</owl:Restriction>
				</owl:intersectionOf>
			</owl:Class>
		</owl:equivalentClass>
		<rdfs:subClassOf rdf:resource="&java;JRE"/>
		<rdfs:comment xml:lang="en">J2ME PP 1.0 Java Runtime Environment</rdfs:comment>
	</owl:Class>
	<owl:Class rdf:about="&j2me-pp-1_0;JavaIo">
		<rdfs:subClassOf rdf:resource="&j2me-midp-2_0;JavaIo"/>
		<rdfs:subClassOf rdf:resource="&j2me-midp-1_0;JavaIo"/>
		<rdfs:seeAlso rdf:resource="&j2me-pp-1_0;JavaSecurity"/>
		<rdfs:seeAlso rdf:resource="&j2me-pp-1_0;JavaUtil"/>
		<rdfs:seeAlso rdf:resource="&j2me-pp-1_0;JavaLang"/>
		<rdfs:seeAlso rdf:resource="&j2me-pp-1_0;JavaNet"/>
		<rdfs:comment xml:lang="en">Java API part implementing the java.io package for J2ME PP 1.0</rdfs:comment>
	</owl:Class>
	<owl:Class rdf:about="&j2me-pp-1_0;JavaLang">
		<rdfs:subClassOf rdf:resource="&j2me-midp-2_0;JavaLang"/>
		<rdfs:subClassOf rdf:resource="&j2me-midp-1_0;JavaLang"/>
		<rdfs:seeAlso rdf:resource="&j2me-pp-1_0;JavaSecurity"/>
		<rdfs:seeAlso rdf:resource="&j2me-pp-1_0;JavaIo"/>
		<rdfs:seeAlso rdf:resource="&j2me-pp-1_0;JavaUtil"/>
		<rdfs:seeAlso rdf:resource="&j2me-pp-1_0;JavaLangReflect"/>
		<rdfs:seeAlso rdf:resource="&j2me-pp-1_0;JavaNet"/>
		<rdfs:comment xml:lang="en">Java API part implementing the java.lang package for J2ME PP 1.0</rdfs:comment>
	</owl:Class>
	<owl:Class rdf:about="&j2me-pp-1_0;JavaLangReflect">
		<rdfs:subClassOf rdf:resource="&j2se-1_2;JavaLangReflect"/>
		<rdfs:seeAlso rdf:resource="&j2me-pp-1_0;JavaSecurity"/>
		<rdfs:seeAlso rdf:resource="&j2me-pp-1_0;JavaIo"/>
		<rdfs:seeAlso rdf:resource="&j2me-pp-1_0;JavaLang"/>
		<rdfs:comment xml:lang="en">Java API part implementing the java.lang.reflect package for J2ME PP 1.0</rdfs:comment>
	</owl:Class>
	<owl:Class rdf:about="&j2me-pp-1_0;JavaLangRef">
		<owl:equivalentClass rdf:resource="&j2se-1_2;JavaLangRef"/>
		<rdfs:subClassOf rdf:resource="&java;JavaAPIPart"/>
		<rdfs:seeAlso rdf:resource="&j2me-pp-1_0;JavaLang"/>
		<rdfs:comment xml:lang="en">Java API part implementing the java.lang.ref package for J2ME PP 1.0</rdfs:comment>
	</owl:Class>
	<owl:Class rdf:about="&j2me-pp-1_0;JavaNet">
		<rdfs:subClassOf rdf:resource="&java;JavaAPIPart"/>
		<rdfs:seeAlso rdf:resource="&j2me-pp-1_0;JavaSecurity"/>
		<rdfs:seeAlso rdf:resource="&j2me-pp-1_0;JavaIo"/>
		<rdfs:seeAlso rdf:resource="&j2me-pp-1_0;JavaUtil"/>
		<rdfs:seeAlso rdf:resource="&j2me-pp-1_0;JavaUtilJar"/>
		<rdfs:seeAlso rdf:resource="&j2me-pp-1_0;JavaLang"/>
		<rdfs:comment xml:lang="en">Java API part implementing the java.net package for J2ME PP 1.0</rdfs:comment>
	</owl:Class>
	<owl:Class rdf:about="&j2me-pp-1_0;JavaSecurity">
		<rdfs:subClassOf rdf:resource="&java;JavaAPIPart"/>
		<rdfs:seeAlso rdf:resource="&j2me-pp-1_0;JavaIo"/>
		<rdfs:seeAlso rdf:resource="&j2me-pp-1_0;JavaSecuritySpec"/>
		<rdfs:seeAlso rdf:resource="&j2me-pp-1_0;JavaUtil"/>
		<rdfs:seeAlso rdf:resource="&j2me-pp-1_0;JavaSecurityCert"/>
		<rdfs:seeAlso rdf:resource="&j2me-pp-1_0;JavaLang"/>
		<rdfs:seeAlso rdf:resource="&j2me-pp-1_0;JavaNet"/>
		<rdfs:comment xml:lang="en">Java API part implementing the java.security package for J2ME PP 1.0</rdfs:comment>
	</owl:Class>
	<owl:Class rdf:about="&j2me-pp-1_0;JavaSecurityCert">
		<rdfs:subClassOf rdf:resource="&j2se-1_2;JavaSecurityCert"/>
		<rdfs:seeAlso rdf:resource="&j2me-pp-1_0;JavaSecurity"/>
		<rdfs:seeAlso rdf:resource="&j2me-pp-1_0;JavaIo"/>
		<rdfs:seeAlso rdf:resource="&j2me-pp-1_0;JavaMath"/>
		<rdfs:seeAlso rdf:resource="&j2me-pp-1_0;JavaUtil"/>
		<rdfs:seeAlso rdf:resource="&j2me-pp-1_0;JavaLang"/>
		<rdfs:comment xml:lang="en">Java API part implementing the java.security.cert package for J2ME PP 1.0</rdfs:comment>
	</owl:Class>
	<owl:Class rdf:about="&j2me-pp-1_0;JavaSecuritySpec">
		<rdfs:subClassOf rdf:resource="&j2se-1_2;JavaSecuritySpec"/>
		<rdfs:seeAlso rdf:resource="&j2me-pp-1_0;JavaSecurity"/>
		<rdfs:seeAlso rdf:resource="&j2me-pp-1_0;JavaMath"/>
		<rdfs:seeAlso rdf:resource="&j2me-pp-1_0;JavaSecurityInterfaces"/>
		<rdfs:seeAlso rdf:resource="&j2me-pp-1_0;JavaLang"/>
		<rdfs:comment xml:lang="en">Java API part implementing the java.security.spec package for J2ME PP 1.0</rdfs:comment>
	</owl:Class>
	<owl:Class rdf:about="&j2me-pp-1_0;JavaSecurityInterfaces">
		<rdfs:subClassOf rdf:resource="&j2se-1_2;JavaSecurityInterfaces"/>
		<rdfs:seeAlso rdf:resource="&j2me-pp-1_0;JavaSecurity"/>
		<rdfs:seeAlso rdf:resource="&j2me-pp-1_0;JavaMath"/>
		<rdfs:comment xml:lang="en">Java API part implementing the java.security.interfaces package for J2ME PP 1.0</rdfs:comment>
	</owl:Class>
	<owl:Class rdf:about="&j2me-pp-1_0;JavaSecurityAcl">
		<owl:equivalentClass rdf:resource="&j2se-1_2;JavaSecurityAcl"/>
		<rdfs:subClassOf rdf:resource="&java;JavaAPIPart"/>
		<rdfs:seeAlso rdf:resource="&j2me-pp-1_0;JavaSecurity"/>
		<rdfs:seeAlso rdf:resource="&j2me-pp-1_0;JavaUtil"/>
		<rdfs:seeAlso rdf:resource="&j2me-pp-1_0;JavaLang"/>
		<rdfs:comment xml:lang="en">Java API part implementing the java.security.acl package for J2ME PP 1.0</rdfs:comment>
	</owl:Class>
	<owl:Class rdf:about="&j2me-pp-1_0;JavaUtil">
		<rdfs:subClassOf rdf:resource="&j2me-midp-2_0;JavaUtil"/>
		<rdfs:subClassOf rdf:resource="&j2me-midp-1_0;JavaUtil"/>
		<rdfs:seeAlso rdf:resource="&j2me-pp-1_0;JavaSecurity"/>
		<rdfs:seeAlso rdf:resource="&j2me-pp-1_0;JavaIo"/>
		<rdfs:seeAlso rdf:resource="&j2me-pp-1_0;JavaLang"/>
		<rdfs:comment xml:lang="en">Java API part implementing the java.util package for J2ME PP 1.0</rdfs:comment>
	</owl:Class>
	<owl:Class rdf:about="&j2me-pp-1_0;JavaUtilJar">
		<rdfs:subClassOf rdf:resource="&j2se-1_2;JavaUtilJar"/>
		<rdfs:seeAlso rdf:resource="&j2me-pp-1_0;JavaIo"/>
		<rdfs:seeAlso rdf:resource="&j2me-pp-1_0;JavaUtil"/>
		<rdfs:seeAlso rdf:resource="&j2me-pp-1_0;JavaUtilZip"/>
		<rdfs:seeAlso rdf:resource="&j2me-pp-1_0;JavaLang"/>
		<rdfs:comment xml:lang="en">Java API part implementing the java.util.jar package for J2ME PP 1.0</rdfs:comment>
	</owl:Class>
	<owl:Class rdf:about="&j2me-pp-1_0;JavaUtilZip">
		<rdfs:subClassOf rdf:resource="&j2se-1_2;JavaUtilZip"/>
		<rdfs:seeAlso rdf:resource="&j2me-pp-1_0;JavaIo"/>
		<rdfs:seeAlso rdf:resource="&j2me-pp-1_0;JavaUtil"/>
		<rdfs:seeAlso rdf:resource="&j2me-pp-1_0;JavaLang"/>
		<rdfs:comment xml:lang="en">Java API part implementing the java.util.zip package for J2ME PP 1.0</rdfs:comment>
	</owl:Class>
	<owl:Class rdf:about="&j2me-pp-1_0;JavaMath">
		<owl:equivalentClass rdf:resource="&j2se-1_2;JavaMath"/>
		<rdfs:subClassOf rdf:resource="&java;JavaAPIPart"/>
		<rdfs:seeAlso rdf:resource="&j2me-pp-1_0;JavaUtil"/>
		<rdfs:seeAlso rdf:resource="&j2me-pp-1_0;JavaLang"/>
		<rdfs:comment xml:lang="en">Java API part implementing the java.math package for J2ME PP 1.0</rdfs:comment>
	</owl:Class>
	<owl:Class rdf:about="&j2me-pp-1_0;JavaText">
		<rdfs:subClassOf rdf:resource="&java;JavaAPIPart"/>
		<rdfs:seeAlso rdf:resource="&j2me-pp-1_0;JavaIo"/>
		<rdfs:seeAlso rdf:resource="&j2me-pp-1_0;JavaUtil"/>
		<rdfs:seeAlso rdf:resource="&j2me-pp-1_0;JavaLang"/>
		<rdfs:comment xml:lang="en">Java API part implementing the java.text package for J2ME PP 1.0</rdfs:comment>
	</owl:Class>
	<owl:Class rdf:about="&j2me-pp-1_0;JavaTextResources">
		<rdfs:subClassOf rdf:resource="&java;JavaAPIPart"/>
		<rdfs:seeAlso rdf:resource="&j2me-pp-1_0;JavaUtil"/>
		<rdfs:seeAlso rdf:resource="&j2me-pp-1_0;JavaLang"/>
		<rdfs:comment xml:lang="en">Java API part implementing the java.text.resources package for J2ME PP 1.0</rdfs:comment>
	</owl:Class>
	<owl:Class rdf:about="&j2me-pp-1_0;JavaApplet">
		<rdfs:subClassOf rdf:resource="&java;JavaAPIPart"/>
		<rdfs:seeAlso rdf:resource="&j2me-pp-1_0;JavaAwt"/>
		<rdfs:seeAlso rdf:resource="&j2me-pp-1_0;JavaUtil"/>
		<rdfs:seeAlso rdf:resource="&j2me-pp-1_0;JavaLang"/>
		<rdfs:seeAlso rdf:resource="&j2me-pp-1_0;JavaNet"/>
		<rdfs:comment xml:lang="en">Java API part implementing the java.applet package for J2ME PP 1.0</rdfs:comment>
	</owl:Class>
	<owl:Class rdf:about="&j2me-pp-1_0;JavaAwt">
		<rdfs:subClassOf rdf:resource="&java;JavaAPIPart"/>
		<rdfs:seeAlso rdf:resource="&j2me-pp-1_0;JavaSecurity"/>
		<rdfs:seeAlso rdf:resource="&j2me-pp-1_0;JavaAwtDatatransfer"/>
		<rdfs:seeAlso rdf:resource="&j2me-pp-1_0;JavaIo"/>
		<rdfs:seeAlso rdf:resource="&j2me-pp-1_0;JavaUtil"/>
		<rdfs:seeAlso rdf:resource="&j2me-pp-1_0;JavaAwtImage"/>
		<rdfs:seeAlso rdf:resource="&j2me-pp-1_0;JavaAwtColor"/>
		<rdfs:seeAlso rdf:resource="&j2me-pp-1_0;JavaLang"/>
		<rdfs:seeAlso rdf:resource="&j2me-pp-1_0;JavaAwtEvent"/>
		<rdfs:seeAlso rdf:resource="&j2me-pp-1_0;JavaNet"/>
		<rdfs:comment xml:lang="en">Java API part implementing the java.awt package for J2ME PP 1.0</rdfs:comment>
	</owl:Class>
	<owl:Class rdf:about="&j2me-pp-1_0;JavaAwtEvent">
		<rdfs:subClassOf rdf:resource="&java;JavaAPIPart"/>
		<rdfs:seeAlso rdf:resource="&j2me-pp-1_0;JavaAwt"/>
		<rdfs:seeAlso rdf:resource="&j2me-pp-1_0;JavaUtil"/>
		<rdfs:seeAlso rdf:resource="&j2me-pp-1_0;JavaLang"/>
		<rdfs:comment xml:lang="en">Java API part implementing the java.awt.event package for J2ME PP 1.0</rdfs:comment>
	</owl:Class>
	<owl:Class rdf:about="&j2me-pp-1_0;JavaAwtImage">
		<rdfs:subClassOf rdf:resource="&java;JavaAPIPart"/>
		<rdfs:seeAlso rdf:resource="&j2me-pp-1_0;JavaAwt"/>
		<rdfs:seeAlso rdf:resource="&j2me-pp-1_0;JavaAwtColor"/>
		<rdfs:seeAlso rdf:resource="&j2me-pp-1_0;JavaUtil"/>
		<rdfs:seeAlso rdf:resource="&j2me-pp-1_0;JavaLang"/>
		<rdfs:comment xml:lang="en">Java API part implementing the java.awt.image package for J2ME PP 1.0</rdfs:comment>
	</owl:Class>
	<owl:Class rdf:about="&j2me-pp-1_0;JavaAwtColor">
		<rdfs:subClassOf rdf:resource="&java;JavaAPIPart"/>
		<rdfs:seeAlso rdf:resource="&j2me-pp-1_0;JavaIo"/>
		<rdfs:seeAlso rdf:resource="&j2me-pp-1_0;JavaLang"/>
		<rdfs:comment xml:lang="en">Java API part implementing the java.awt.color package for J2ME PP 1.0</rdfs:comment>
	</owl:Class>
	<owl:Class rdf:about="&j2me-pp-1_0;JavaAwtDatatransfer">
		<rdfs:subClassOf rdf:resource="&java;JavaAPIPart"/>
		<rdfs:seeAlso rdf:resource="&j2me-pp-1_0;JavaIo"/>
		<rdfs:seeAlso rdf:resource="&j2me-pp-1_0;JavaLang"/>
		<rdfs:comment xml:lang="en">Java API part implementing the java.awt.datatransfer package for J2ME PP 1.0</rdfs:comment>
	</owl:Class>
	<owl:Class rdf:about="&j2me-pp-1_0;JavaBeans">
		<rdfs:subClassOf rdf:resource="&java;JavaAPIPart"/>
		<rdfs:seeAlso rdf:resource="&j2me-pp-1_0;JavaIo"/>
		<rdfs:seeAlso rdf:resource="&j2me-pp-1_0;JavaUtil"/>
		<rdfs:seeAlso rdf:resource="&j2me-pp-1_0;JavaLang"/>
		<rdfs:comment xml:lang="en">Java API part implementing the java.beans package for J2ME PP 1.0</rdfs:comment>
	</owl:Class>
	<owl:Class rdf:about="&j2me-pp-1_0;JavaRmi">
		<rdfs:subClassOf rdf:resource="&java;JavaAPIPart"/>
		<rdfs:seeAlso rdf:resource="&j2me-pp-1_0;JavaIo"/>
		<rdfs:seeAlso rdf:resource="&j2me-pp-1_0;JavaLang"/>
		<rdfs:comment xml:lang="en">Java API part implementing the java.rmi package for J2ME PP 1.0</rdfs:comment>
	</owl:Class>
	<owl:Class rdf:about="&j2me-pp-1_0;JavaRmiRegistry">
		<rdfs:subClassOf rdf:resource="&java;JavaAPIPart"/>
		<rdfs:seeAlso rdf:resource="&j2me-pp-1_0;JavaLang"/>
		<rdfs:seeAlso rdf:resource="&j2me-pp-1_0;JavaRmi"/>
		<rdfs:comment xml:lang="en">Java API part implementing the java.rmi.registry package for J2ME PP 1.0</rdfs:comment>
	</owl:Class>
	<owl:Class rdf:about="&j2me-pp-1_0;JavaxMicroeditionIo">
		<rdfs:subClassOf rdf:resource="&j2me-midp-1_0;JavaxMicroeditionIo"/>
		<rdfs:seeAlso rdf:resource="&j2me-pp-1_0;JavaIo"/>
		<rdfs:seeAlso rdf:resource="&j2me-pp-1_0;JavaLang"/>
		<rdfs:comment xml:lang="en">Java API part implementing the javax.microedition.io package for J2ME PP 1.0</rdfs:comment>
	</owl:Class>
	<owl:Class rdf:about="&j2me-pp-1_0;JavaxMicroeditionXlet">
		<rdfs:subClassOf rdf:resource="&java;JavaAPIPart"/>
		<rdfs:seeAlso rdf:resource="&j2me-pp-1_0;JavaAwt"/>
		<rdfs:seeAlso rdf:resource="&j2me-pp-1_0;JavaLang"/>
		<rdfs:comment xml:lang="en">Java API part implementing the javax.microedition.xlet package for J2ME PP 1.0</rdfs:comment>
	</owl:Class>
	<owl:Class rdf:about="&j2me-pp-1_0;JavaxMicroeditionXletIxc">
		<rdfs:subClassOf rdf:resource="&java;JavaAPIPart"/>
		<rdfs:seeAlso rdf:resource="&j2me-pp-1_0;JavaxMicroeditionXlet"/>
		<rdfs:seeAlso rdf:resource="&j2me-pp-1_0;JavaRmiRegistry"/>
		<rdfs:seeAlso rdf:resource="&j2me-pp-1_0;JavaRmi"/>
		<rdfs:seeAlso rdf:resource="&j2me-pp-1_0;JavaLang"/>
		<rdfs:comment xml:lang="en">Java API part implementing the javax.microedition.xlet.ixc package for J2ME PP 1.0</rdfs:comment>
	</owl:Class>
	<owl:Class rdf:about="&j2me-pp-1_0;JavaIoAPI">
		<rdfs:subClassOf rdf:resource="&j2me-midp-2_0;JavaIoAPI"/>
		<rdfs:subClassOf rdf:resource="&j2me-midp-1_0;JavaIoAPI"/>
		<rdfs:comment xml:lang="en">JavaLibrary implementing the java.io package for J2ME PP 1.0</rdfs:comment>
		<rdfs:comment xml:lang="OWLManchester">platform:comprisesInterfacePart some JavaIo</rdfs:comment>
	</owl:Class>
	<owl:Class rdf:about="&j2me-pp-1_0;JavaLangAPI">
		<rdfs:subClassOf rdf:resource="&j2me-midp-2_0;JavaLangAPI"/>
		<rdfs:subClassOf rdf:resource="&j2me-midp-1_0;JavaLangAPI"/>
		<rdfs:comment xml:lang="en">JavaLibrary implementing the java.lang package for J2ME PP 1.0</rdfs:comment>
		<rdfs:comment xml:lang="OWLManchester">platform:comprisesInterfacePart some JavaLang</rdfs:comment>
	</owl:Class>
	<owl:Class rdf:about="&j2me-pp-1_0;JavaLangReflectAPI">
		<rdfs:subClassOf rdf:resource="&j2se-1_2;JavaLangReflectAPI"/>
		<rdfs:comment xml:lang="en">JavaLibrary implementing the java.lang.reflect package for J2ME PP 1.0</rdfs:comment>
		<rdfs:comment xml:lang="OWLManchester">platform:comprisesInterfacePart some JavaLangReflect</rdfs:comment>
	</owl:Class>
	<owl:Class rdf:about="&j2me-pp-1_0;JavaLangRefAPI">
		<owl:equivalentClass rdf:resource="&j2se-1_2;JavaLangRefAPI"/>
		<rdfs:subClassOf rdf:resource="&java;JavaAPI"/>
		<rdfs:comment xml:lang="en">JavaLibrary implementing the java.lang.ref package for J2ME PP 1.0</rdfs:comment>
		<rdfs:comment xml:lang="OWLManchester">platform:comprisesInterfacePart some JavaLangRef</rdfs:comment>
	</owl:Class>
	<owl:Class rdf:about="&j2me-pp-1_0;JavaNetAPI">
		<rdfs:subClassOf rdf:resource="&java;JavaAPI"/>
		<rdfs:comment xml:lang="en">JavaLibrary implementing the java.net package for J2ME PP 1.0</rdfs:comment>
		<rdfs:comment xml:lang="OWLManchester">platform:comprisesInterfacePart some JavaNet</rdfs:comment>
	</owl:Class>
	<owl:Class rdf:about="&j2me-pp-1_0;JavaSecurityAPI">
		<rdfs:subClassOf rdf:resource="&java;JavaAPI"/>
		<rdfs:comment xml:lang="en">JavaLibrary implementing the java.security package for J2ME PP 1.0</rdfs:comment>
		<rdfs:comment xml:lang="OWLManchester">platform:comprisesInterfacePart some JavaSecurity</rdfs:comment>
	</owl:Class>
	<owl:Class rdf:about="&j2me-pp-1_0;JavaSecurityCertAPI">
		<rdfs:subClassOf rdf:resource="&j2se-1_2;JavaSecurityCertAPI"/>
		<rdfs:comment xml:lang="en">JavaLibrary implementing the java.security.cert package for J2ME PP 1.0</rdfs:comment>
		<rdfs:comment xml:lang="OWLManchester">platform:comprisesInterfacePart some JavaSecurityCert</rdfs:comment>
	</owl:Class>
	<owl:Class rdf:about="&j2me-pp-1_0;JavaSecuritySpecAPI">
		<rdfs:subClassOf rdf:resource="&j2se-1_2;JavaSecuritySpecAPI"/>
		<rdfs:comment xml:lang="en">JavaLibrary implementing the java.security.spec package for J2ME PP 1.0</rdfs:comment>
		<rdfs:comment xml:lang="OWLManchester">platform:comprisesInterfacePart some JavaSecuritySpec</rdfs:comment>
	</owl:Class>
	<owl:Class rdf:about="&j2me-pp-1_0;JavaSecurityInterfacesAPI">
		<rdfs:subClassOf rdf:resource="&j2se-1_2;JavaSecurityInterfacesAPI"/>
		<rdfs:comment xml:lang="en">JavaLibrary implementing the java.security.interfaces package for J2ME PP 1.0</rdfs:comment>
		<rdfs:comment xml:lang="OWLManchester">platform:comprisesInterfacePart some JavaSecurityInterfaces</rdfs:comment>
	</owl:Class>
	<owl:Class rdf:about="&j2me-pp-1_0;JavaSecurityAclAPI">
		<owl:equivalentClass rdf:resource="&j2se-1_2;JavaSecurityAclAPI"/>
		<rdfs:subClassOf rdf:resource="&java;JavaAPI"/>
		<rdfs:comment xml:lang="en">JavaLibrary implementing the java.security.acl package for J2ME PP 1.0</rdfs:comment>
		<rdfs:comment xml:lang="OWLManchester">platform:comprisesInterfacePart some JavaSecurityAcl</rdfs:comment>
	</owl:Class>
	<owl:Class rdf:about="&j2me-pp-1_0;JavaUtilAPI">
		<rdfs:subClassOf rdf:resource="&j2me-midp-2_0;JavaUtilAPI"/>
		<rdfs:subClassOf rdf:resource="&j2me-midp-1_0;JavaUtilAPI"/>
		<rdfs:comment xml:lang="en">JavaLibrary implementing the java.util package for J2ME PP 1.0</rdfs:comment>
		<rdfs:comment xml:lang="OWLManchester">platform:comprisesInterfacePart some JavaUtil</rdfs:comment>
	</owl:Class>
	<owl:Class rdf:about="&j2me-pp-1_0;JavaUtilJarAPI">
		<rdfs:subClassOf rdf:resource="&j2se-1_2;JavaUtilJarAPI"/>
		<rdfs:comment xml:lang="en">JavaLibrary implementing the java.util.jar package for J2ME PP 1.0</rdfs:comment>
		<rdfs:comment xml:lang="OWLManchester">platform:comprisesInterfacePart some JavaUtilJar</rdfs:comment>
	</owl:Class>
	<owl:Class rdf:about="&j2me-pp-1_0;JavaUtilZipAPI">
		<rdfs:subClassOf rdf:resource="&j2se-1_2;JavaUtilZipAPI"/>
		<rdfs:comment xml:lang="en">JavaLibrary implementing the java.util.zip package for J2ME PP 1.0</rdfs:comment>
		<rdfs:comment xml:lang="OWLManchester">platform:comprisesInterfacePart some JavaUtilZip</rdfs:comment>
	</owl:Class>
	<owl:Class rdf:about="&j2me-pp-1_0;JavaMathAPI">
		<owl:equivalentClass rdf:resource="&j2se-1_2;JavaMathAPI"/>
		<rdfs:subClassOf rdf:resource="&java;JavaAPI"/>
		<rdfs:comment xml:lang="en">JavaLibrary implementing the java.math package for J2ME PP 1.0</rdfs:comment>
		<rdfs:comment xml:lang="OWLManchester">platform:comprisesInterfacePart some JavaMath</rdfs:comment>
	</owl:Class>
	<owl:Class rdf:about="&j2me-pp-1_0;JavaTextAPI">
		<rdfs:subClassOf rdf:resource="&java;JavaAPI"/>
		<rdfs:comment xml:lang="en">JavaLibrary implementing the java.text package for J2ME PP 1.0</rdfs:comment>
		<rdfs:comment xml:lang="OWLManchester">platform:comprisesInterfacePart some JavaText</rdfs:comment>
	</owl:Class>
	<owl:Class rdf:about="&j2me-pp-1_0;JavaTextResourcesAPI">
		<rdfs:subClassOf rdf:resource="&java;JavaAPI"/>
		<rdfs:comment xml:lang="en">JavaLibrary implementing the java.text.resources package for J2ME PP 1.0</rdfs:comment>
		<rdfs:comment xml:lang="OWLManchester">platform:comprisesInterfacePart some JavaTextResources</rdfs:comment>
	</owl:Class>
	<owl:Class rdf:about="&j2me-pp-1_0;JavaAppletAPI">
		<rdfs:subClassOf rdf:resource="&java;JavaAPI"/>
		<rdfs:comment xml:lang="en">JavaLibrary implementing the java.applet package for J2ME PP 1.0</rdfs:comment>
		<rdfs:comment xml:lang="OWLManchester">platform:comprisesInterfacePart some JavaApplet</rdfs:comment>
	</owl:Class>
	<owl:Class rdf:about="&j2me-pp-1_0;JavaAwtAPI">
		<rdfs:subClassOf rdf:resource="&java;JavaAPI"/>
		<rdfs:comment xml:lang="en">JavaLibrary implementing the java.awt package for J2ME PP 1.0</rdfs:comment>
		<rdfs:comment xml:lang="OWLManchester">platform:comprisesInterfacePart some JavaAwt</rdfs:comment>
	</owl:Class>
	<owl:Class rdf:about="&j2me-pp-1_0;JavaAwtEventAPI">
		<rdfs:subClassOf rdf:resource="&java;JavaAPI"/>
		<rdfs:comment xml:lang="en">JavaLibrary implementing the java.awt.event package for J2ME PP 1.0</rdfs:comment>
		<rdfs:comment xml:lang="OWLManchester">platform:comprisesInterfacePart some JavaAwtEvent</rdfs:comment>
	</owl:Class>
	<owl:Class rdf:about="&j2me-pp-1_0;JavaAwtImageAPI">
		<rdfs:subClassOf rdf:resource="&java;JavaAPI"/>
		<rdfs:comment xml:lang="en">JavaLibrary implementing the java.awt.image package for J2ME PP 1.0</rdfs:comment>
		<rdfs:comment xml:lang="OWLManchester">platform:comprisesInterfacePart some JavaAwtImage</rdfs:comment>
	</owl:Class>
	<owl:Class rdf:about="&j2me-pp-1_0;JavaAwtColorAPI">
		<rdfs:subClassOf rdf:resource="&java;JavaAPI"/>
		<rdfs:comment xml:lang="en">JavaLibrary implementing the java.awt.color package for J2ME PP 1.0</rdfs:comment>
		<rdfs:comment xml:lang="OWLManchester">platform:comprisesInterfacePart some JavaAwtColor</rdfs:comment>
	</owl:Class>
	<owl:Class rdf:about="&j2me-pp-1_0;JavaAwtDatatransferAPI">
		<rdfs:subClassOf rdf:resource="&java;JavaAPI"/>
		<rdfs:comment xml:lang="en">JavaLibrary implementing the java.awt.datatransfer package for J2ME PP 1.0</rdfs:comment>
		<rdfs:comment xml:lang="OWLManchester">platform:comprisesInterfacePart some JavaAwtDatatransfer</rdfs:comment>
	</owl:Class>
	<owl:Class rdf:about="&j2me-pp-1_0;JavaBeansAPI">
		<rdfs:subClassOf rdf:resource="&java;JavaAPI"/>
		<rdfs:comment xml:lang="en">JavaLibrary implementing the java.beans package for J2ME PP 1.0</rdfs:comment>
		<rdfs:comment xml:lang="OWLManchester">platform:comprisesInterfacePart some JavaBeans</rdfs:comment>
	</owl:Class>
	<owl:Class rdf:about="&j2me-pp-1_0;JavaRmiAPI">
		<rdfs:subClassOf rdf:resource="&java;JavaAPI"/>
		<rdfs:comment xml:lang="en">JavaLibrary implementing the java.rmi package for J2ME PP 1.0</rdfs:comment>
		<rdfs:comment xml:lang="OWLManchester">platform:comprisesInterfacePart some JavaRmi</rdfs:comment>
	</owl:Class>
	<owl:Class rdf:about="&j2me-pp-1_0;JavaRmiRegistryAPI">
		<rdfs:subClassOf rdf:resource="&java;JavaAPI"/>
		<rdfs:comment xml:lang="en">JavaLibrary implementing the java.rmi.registry package for J2ME PP 1.0</rdfs:comment>
		<rdfs:comment xml:lang="OWLManchester">platform:comprisesInterfacePart some JavaRmiRegistry</rdfs:comment>
	</owl:Class>
	<owl:Class rdf:about="&j2me-pp-1_0;JavaxMicroeditionIoAPI">
		<rdfs:subClassOf rdf:resource="&j2me-midp-1_0;JavaxMicroeditionIoAPI"/>
		<rdfs:comment xml:lang="en">JavaLibrary implementing the javax.microedition.io package for J2ME PP 1.0</rdfs:comment>
		<rdfs:comment xml:lang="OWLManchester">platform:comprisesInterfacePart some JavaxMicroeditionIo</rdfs:comment>
	</owl:Class>
	<owl:Class rdf:about="&j2me-pp-1_0;JavaxMicroeditionXletAPI">
		<rdfs:subClassOf rdf:resource="&java;JavaAPI"/>
		<rdfs:comment xml:lang="en">JavaLibrary implementing the javax.microedition.xlet package for J2ME PP 1.0</rdfs:comment>
		<rdfs:comment xml:lang="OWLManchester">platform:comprisesInterfacePart some JavaxMicroeditionXlet</rdfs:comment>
	</owl:Class>
	<owl:Class rdf:about="&j2me-pp-1_0;JavaxMicroeditionXletIxcAPI">
		<rdfs:subClassOf rdf:resource="&java;JavaAPI"/>
		<rdfs:comment xml:lang="en">JavaLibrary implementing the javax.microedition.xlet.ixc package for J2ME PP 1.0</rdfs:comment>
		<rdfs:comment xml:lang="OWLManchester">platform:comprisesInterfacePart some JavaxMicroeditionXletIxc</rdfs:comment>
	</owl:Class>
	<j2me-pp-1_0:JavaIo rdf:about="&j2me-pp-1_0;theJavaIoPart">
	</j2me-pp-1_0:JavaIo>
	<j2me-pp-1_0:JavaLang rdf:about="&j2me-pp-1_0;theJavaLangPart">
	</j2me-pp-1_0:JavaLang>
	<j2me-pp-1_0:JavaLangReflect rdf:about="&j2me-pp-1_0;theJavaLangReflectPart">
	</j2me-pp-1_0:JavaLangReflect>
	<j2me-pp-1_0:JavaLangRef rdf:about="&j2me-pp-1_0;theJavaLangRefPart">
	</j2me-pp-1_0:JavaLangRef>
	<j2me-pp-1_0:JavaNet rdf:about="&j2me-pp-1_0;theJavaNetPart">
	</j2me-pp-1_0:JavaNet>
	<j2me-pp-1_0:JavaSecurity rdf:about="&j2me-pp-1_0;theJavaSecurityPart">
	</j2me-pp-1_0:JavaSecurity>
	<j2me-pp-1_0:JavaSecurityCert rdf:about="&j2me-pp-1_0;theJavaSecurityCertPart">
	</j2me-pp-1_0:JavaSecurityCert>
	<j2me-pp-1_0:JavaSecuritySpec rdf:about="&j2me-pp-1_0;theJavaSecuritySpecPart">
	</j2me-pp-1_0:JavaSecuritySpec>
	<j2me-pp-1_0:JavaSecurityInterfaces rdf:about="&j2me-pp-1_0;theJavaSecurityInterfacesPart">
	</j2me-pp-1_0:JavaSecurityInterfaces>
	<j2me-pp-1_0:JavaSecurityAcl rdf:about="&j2me-pp-1_0;theJavaSecurityAclPart">
	</j2me-pp-1_0:JavaSecurityAcl>
	<j2me-pp-1_0:JavaUtil rdf:about="&j2me-pp-1_0;theJavaUtilPart">
	</j2me-pp-1_0:JavaUtil>
	<j2me-pp-1_0:JavaUtilJar rdf:about="&j2me-pp-1_0;theJavaUtilJarPart">
	</j2me-pp-1_0:JavaUtilJar>
	<j2me-pp-1_0:JavaUtilZip rdf:about="&j2me-pp-1_0;theJavaUtilZipPart">
	</j2me-pp-1_0:JavaUtilZip>
	<j2me-pp-1_0:JavaMath rdf:about="&j2me-pp-1_0;theJavaMathPart">
	</j2me-pp-1_0:JavaMath>
	<j2me-pp-1_0:JavaText rdf:about="&j2me-pp-1_0;theJavaTextPart">
	</j2me-pp-1_0:JavaText>
	<j2me-pp-1_0:JavaTextResources rdf:about="&j2me-pp-1_0;theJavaTextResourcesPart">
	</j2me-pp-1_0:JavaTextResources>
	<j2me-pp-1_0:JavaApplet rdf:about="&j2me-pp-1_0;theJavaAppletPart">
	</j2me-pp-1_0:JavaApplet>
	<j2me-pp-1_0:JavaAwt rdf:about="&j2me-pp-1_0;theJavaAwtPart">
	</j2me-pp-1_0:JavaAwt>
	<j2me-pp-1_0:JavaAwtEvent rdf:about="&j2me-pp-1_0;theJavaAwtEventPart">
	</j2me-pp-1_0:JavaAwtEvent>
	<j2me-pp-1_0:JavaAwtImage rdf:about="&j2me-pp-1_0;theJavaAwtImagePart">
	</j2me-pp-1_0:JavaAwtImage>
	<j2me-pp-1_0:JavaAwtColor rdf:about="&j2me-pp-1_0;theJavaAwtColorPart">
	</j2me-pp-1_0:JavaAwtColor>
	<j2me-pp-1_0:JavaAwtDatatransfer rdf:about="&j2me-pp-1_0;theJavaAwtDatatransferPart">
	</j2me-pp-1_0:JavaAwtDatatransfer>
	<j2me-pp-1_0:JavaBeans rdf:about="&j2me-pp-1_0;theJavaBeansPart">
	</j2me-pp-1_0:JavaBeans>
	<j2me-pp-1_0:JavaRmi rdf:about="&j2me-pp-1_0;theJavaRmiPart">
	</j2me-pp-1_0:JavaRmi>
	<j2me-pp-1_0:JavaRmiRegistry rdf:about="&j2me-pp-1_0;theJavaRmiRegistryPart">
	</j2me-pp-1_0:JavaRmiRegistry>
	<j2me-pp-1_0:JavaxMicroeditionIo rdf:about="&j2me-pp-1_0;theJavaxMicroeditionIoPart">
	</j2me-pp-1_0:JavaxMicroeditionIo>
	<j2me-pp-1_0:JavaxMicroeditionXlet rdf:about="&j2me-pp-1_0;theJavaxMicroeditionXletPart">
	</j2me-pp-1_0:JavaxMicroeditionXlet>
	<j2me-pp-1_0:JavaxMicroeditionXletIxc rdf:about="&j2me-pp-1_0;theJavaxMicroeditionXletIxcPart">
	</j2me-pp-1_0:JavaxMicroeditionXletIxc>
	<owl:Class rdf:about="&j2me-pp-1_0;JavaIoClassLibrary">
		<rdfs:subClassOf rdf:resource="&j2me-midp-2_0;JavaIoClassLibrary"/>
		<rdfs:subClassOf rdf:resource="&j2me-midp-1_0;JavaIoClassLibrary"/>
		<rdfs:comment xml:lang="en">JavaLibrary implementing the java.io package for J2ME PP 1.0</rdfs:comment>
		<rdfs:comment xml:lang="OWLManchester">platform:implementsInterface some JavaIoAPI</rdfs:comment>
	</owl:Class>
	<owl:Class rdf:about="&j2me-pp-1_0;JavaLangClassLibrary">
		<rdfs:subClassOf rdf:resource="&j2me-midp-2_0;JavaLangClassLibrary"/>
		<rdfs:subClassOf rdf:resource="&j2me-midp-1_0;JavaLangClassLibrary"/>
		<rdfs:comment xml:lang="en">JavaLibrary implementing the java.lang package for J2ME PP 1.0</rdfs:comment>
		<rdfs:comment xml:lang="OWLManchester">platform:implementsInterface some JavaLangAPI</rdfs:comment>
	</owl:Class>
	<owl:Class rdf:about="&j2me-pp-1_0;JavaLangReflectClassLibrary">
		<rdfs:subClassOf rdf:resource="&j2se-1_2;JavaLangReflectClassLibrary"/>
		<rdfs:comment xml:lang="en">JavaLibrary implementing the java.lang.reflect package for J2ME PP 1.0</rdfs:comment>
		<rdfs:comment xml:lang="OWLManchester">platform:implementsInterface some JavaLangReflectAPI</rdfs:comment>
	</owl:Class>
	<owl:Class rdf:about="&j2me-pp-1_0;JavaLangRefClassLibrary">
		<owl:equivalentClass rdf:resource="&j2se-1_2;JavaLangRefClassLibrary"/>
		<rdfs:subClassOf rdf:resource="&java;JavaClassLibrary"/>
		<rdfs:comment xml:lang="en">JavaLibrary implementing the java.lang.ref package for J2ME PP 1.0</rdfs:comment>
		<rdfs:comment xml:lang="OWLManchester">platform:implementsInterface some JavaLangRefAPI</rdfs:comment>
	</owl:Class>
	<owl:Class rdf:about="&j2me-pp-1_0;JavaNetClassLibrary">
		<rdfs:subClassOf rdf:resource="&java;JavaClassLibrary"/>
		<rdfs:comment xml:lang="en">JavaLibrary implementing the java.net package for J2ME PP 1.0</rdfs:comment>
		<rdfs:comment xml:lang="OWLManchester">platform:implementsInterface some JavaNetAPI</rdfs:comment>
	</owl:Class>
	<owl:Class rdf:about="&j2me-pp-1_0;JavaSecurityClassLibrary">
		<rdfs:subClassOf rdf:resource="&java;JavaClassLibrary"/>
		<rdfs:comment xml:lang="en">JavaLibrary implementing the java.security package for J2ME PP 1.0</rdfs:comment>
		<rdfs:comment xml:lang="OWLManchester">platform:implementsInterface some JavaSecurityAPI</rdfs:comment>
	</owl:Class>
	<owl:Class rdf:about="&j2me-pp-1_0;JavaSecurityCertClassLibrary">
		<rdfs:subClassOf rdf:resource="&j2se-1_2;JavaSecurityCertClassLibrary"/>
		<rdfs:comment xml:lang="en">JavaLibrary implementing the java.security.cert package for J2ME PP 1.0</rdfs:comment>
		<rdfs:comment xml:lang="OWLManchester">platform:implementsInterface some JavaSecurityCertAPI</rdfs:comment>
	</owl:Class>
	<owl:Class rdf:about="&j2me-pp-1_0;JavaSecuritySpecClassLibrary">
		<rdfs:subClassOf rdf:resource="&j2se-1_2;JavaSecuritySpecClassLibrary"/>
		<rdfs:comment xml:lang="en">JavaLibrary implementing the java.security.spec package for J2ME PP 1.0</rdfs:comment>
		<rdfs:comment xml:lang="OWLManchester">platform:implementsInterface some JavaSecuritySpecAPI</rdfs:comment>
	</owl:Class>
	<owl:Class rdf:about="&j2me-pp-1_0;JavaSecurityInterfacesClassLibrary">
		<rdfs:subClassOf rdf:resource="&j2se-1_2;JavaSecurityInterfacesClassLibrary"/>
		<rdfs:comment xml:lang="en">JavaLibrary implementing the java.security.interfaces package for J2ME PP 1.0</rdfs:comment>
		<rdfs:comment xml:lang="OWLManchester">platform:implementsInterface some JavaSecurityInterfacesAPI</rdfs:comment>
	</owl:Class>
	<owl:Class rdf:about="&j2me-pp-1_0;JavaSecurityAclClassLibrary">
		<owl:equivalentClass rdf:resource="&j2se-1_2;JavaSecurityAclClassLibrary"/>
		<rdfs:subClassOf rdf:resource="&java;JavaClassLibrary"/>
		<rdfs:comment xml:lang="en">JavaLibrary implementing the java.security.acl package for J2ME PP 1.0</rdfs:comment>
		<rdfs:comment xml:lang="OWLManchester">platform:implementsInterface some JavaSecurityAclAPI</rdfs:comment>
	</owl:Class>
	<owl:Class rdf:about="&j2me-pp-1_0;JavaUtilClassLibrary">
		<rdfs:subClassOf rdf:resource="&j2me-midp-2_0;JavaUtilClassLibrary"/>
		<rdfs:subClassOf rdf:resource="&j2me-midp-1_0;JavaUtilClassLibrary"/>
		<rdfs:comment xml:lang="en">JavaLibrary implementing the java.util package for J2ME PP 1.0</rdfs:comment>
		<rdfs:comment xml:lang="OWLManchester">platform:implementsInterface some JavaUtilAPI</rdfs:comment>
	</owl:Class>
	<owl:Class rdf:about="&j2me-pp-1_0;JavaUtilJarClassLibrary">
		<rdfs:subClassOf rdf:resource="&j2se-1_2;JavaUtilJarClassLibrary"/>
		<rdfs:comment xml:lang="en">JavaLibrary implementing the java.util.jar package for J2ME PP 1.0</rdfs:comment>
		<rdfs:comment xml:lang="OWLManchester">platform:implementsInterface some JavaUtilJarAPI</rdfs:comment>
	</owl:Class>
	<owl:Class rdf:about="&j2me-pp-1_0;JavaUtilZipClassLibrary">
		<rdfs:subClassOf rdf:resource="&j2se-1_2;JavaUtilZipClassLibrary"/>
		<rdfs:comment xml:lang="en">JavaLibrary implementing the java.util.zip package for J2ME PP 1.0</rdfs:comment>
		<rdfs:comment xml:lang="OWLManchester">platform:implementsInterface some JavaUtilZipAPI</rdfs:comment>
	</owl:Class>
	<owl:Class rdf:about="&j2me-pp-1_0;JavaMathClassLibrary">
		<owl:equivalentClass rdf:resource="&j2se-1_2;JavaMathClassLibrary"/>
		<rdfs:subClassOf rdf:resource="&java;JavaClassLibrary"/>
		<rdfs:comment xml:lang="en">JavaLibrary implementing the java.math package for J2ME PP 1.0</rdfs:comment>
		<rdfs:comment xml:lang="OWLManchester">platform:implementsInterface some JavaMathAPI</rdfs:comment>
	</owl:Class>
	<owl:Class rdf:about="&j2me-pp-1_0;JavaTextClassLibrary">
		<rdfs:subClassOf rdf:resource="&java;JavaClassLibrary"/>
		<rdfs:comment xml:lang="en">JavaLibrary implementing the java.text package for J2ME PP 1.0</rdfs:comment>
		<rdfs:comment xml:lang="OWLManchester">platform:implementsInterface some JavaTextAPI</rdfs:comment>
	</owl:Class>
	<owl:Class rdf:about="&j2me-pp-1_0;JavaTextResourcesClassLibrary">
		<rdfs:subClassOf rdf:resource="&java;JavaClassLibrary"/>
		<rdfs:comment xml:lang="en">JavaLibrary implementing the java.text.resources package for J2ME PP 1.0</rdfs:comment>
		<rdfs:comment xml:lang="OWLManchester">platform:implementsInterface some JavaTextResourcesAPI</rdfs:comment>
	</owl:Class>
	<owl:Class rdf:about="&j2me-pp-1_0;JavaAppletClassLibrary">
		<rdfs:subClassOf rdf:resource="&java;JavaClassLibrary"/>
		<rdfs:comment xml:lang="en">JavaLibrary implementing the java.applet package for J2ME PP 1.0</rdfs:comment>
		<rdfs:comment xml:lang="OWLManchester">platform:implementsInterface some JavaAppletAPI</rdfs:comment>
	</owl:Class>
	<owl:Class rdf:about="&j2me-pp-1_0;JavaAwtClassLibrary">
		<rdfs:subClassOf rdf:resource="&java;JavaClassLibrary"/>
		<rdfs:comment xml:lang="en">JavaLibrary implementing the java.awt package for J2ME PP 1.0</rdfs:comment>
		<rdfs:comment xml:lang="OWLManchester">platform:implementsInterface some JavaAwtAPI</rdfs:comment>
	</owl:Class>
	<owl:Class rdf:about="&j2me-pp-1_0;JavaAwtEventClassLibrary">
		<rdfs:subClassOf rdf:resource="&java;JavaClassLibrary"/>
		<rdfs:comment xml:lang="en">JavaLibrary implementing the java.awt.event package for J2ME PP 1.0</rdfs:comment>
		<rdfs:comment xml:lang="OWLManchester">platform:implementsInterface some JavaAwtEventAPI</rdfs:comment>
	</owl:Class>
	<owl:Class rdf:about="&j2me-pp-1_0;JavaAwtImageClassLibrary">
		<rdfs:subClassOf rdf:resource="&java;JavaClassLibrary"/>
		<rdfs:comment xml:lang="en">JavaLibrary implementing the java.awt.image package for J2ME PP 1.0</rdfs:comment>
		<rdfs:comment xml:lang="OWLManchester">platform:implementsInterface some JavaAwtImageAPI</rdfs:comment>
	</owl:Class>
	<owl:Class rdf:about="&j2me-pp-1_0;JavaAwtColorClassLibrary">
		<rdfs:subClassOf rdf:resource="&java;JavaClassLibrary"/>
		<rdfs:comment xml:lang="en">JavaLibrary implementing the java.awt.color package for J2ME PP 1.0</rdfs:comment>
		<rdfs:comment xml:lang="OWLManchester">platform:implementsInterface some JavaAwtColorAPI</rdfs:comment>
	</owl:Class>
	<owl:Class rdf:about="&j2me-pp-1_0;JavaAwtDatatransferClassLibrary">
		<rdfs:subClassOf rdf:resource="&java;JavaClassLibrary"/>
		<rdfs:comment xml:lang="en">JavaLibrary implementing the java.awt.datatransfer package for J2ME PP 1.0</rdfs:comment>
		<rdfs:comment xml:lang="OWLManchester">platform:implementsInterface some JavaAwtDatatransferAPI</rdfs:comment>
	</owl:Class>
	<owl:Class rdf:about="&j2me-pp-1_0;JavaBeansClassLibrary">
		<rdfs:subClassOf rdf:resource="&java;JavaClassLibrary"/>
		<rdfs:comment xml:lang="en">JavaLibrary implementing the java.beans package for J2ME PP 1.0</rdfs:comment>
		<rdfs:comment xml:lang="OWLManchester">platform:implementsInterface some JavaBeansAPI</rdfs:comment>
	</owl:Class>
	<owl:Class rdf:about="&j2me-pp-1_0;JavaRmiClassLibrary">
		<rdfs:subClassOf rdf:resource="&java;JavaClassLibrary"/>
		<rdfs:comment xml:lang="en">JavaLibrary implementing the java.rmi package for J2ME PP 1.0</rdfs:comment>
		<rdfs:comment xml:lang="OWLManchester">platform:implementsInterface some JavaRmiAPI</rdfs:comment>
	</owl:Class>
	<owl:Class rdf:about="&j2me-pp-1_0;JavaRmiRegistryClassLibrary">
		<rdfs:subClassOf rdf:resource="&java;JavaClassLibrary"/>
		<rdfs:comment xml:lang="en">JavaLibrary implementing the java.rmi.registry package for J2ME PP 1.0</rdfs:comment>
		<rdfs:comment xml:lang="OWLManchester">platform:implementsInterface some JavaRmiRegistryAPI</rdfs:comment>
	</owl:Class>
	<owl:Class rdf:about="&j2me-pp-1_0;JavaxMicroeditionIoClassLibrary">
		<rdfs:subClassOf rdf:resource="&j2me-midp-1_0;JavaxMicroeditionIoClassLibrary"/>
		<rdfs:comment xml:lang="en">JavaLibrary implementing the javax.microedition.io package for J2ME PP 1.0</rdfs:comment>
		<rdfs:comment xml:lang="OWLManchester">platform:implementsInterface some JavaxMicroeditionIoAPI</rdfs:comment>
	</owl:Class>
	<owl:Class rdf:about="&j2me-pp-1_0;JavaxMicroeditionXletClassLibrary">
		<rdfs:subClassOf rdf:resource="&java;JavaClassLibrary"/>
		<rdfs:comment xml:lang="en">JavaLibrary implementing the javax.microedition.xlet package for J2ME PP 1.0</rdfs:comment>
		<rdfs:comment xml:lang="OWLManchester">platform:implementsInterface some JavaxMicroeditionXletAPI</rdfs:comment>
	</owl:Class>
	<owl:Class rdf:about="&j2me-pp-1_0;JavaxMicroeditionXletIxcClassLibrary">
		<rdfs:subClassOf rdf:resource="&java;JavaClassLibrary"/>
		<rdfs:comment xml:lang="en">JavaLibrary implementing the javax.microedition.xlet.ixc package for J2ME PP 1.0</rdfs:comment>
		<rdfs:comment xml:lang="OWLManchester">platform:implementsInterface some JavaxMicroeditionXletIxcAPI</rdfs:comment>
	</owl:Class>
</rdf:RDF>
