<?xml version="1.0" encoding="ISO-8859-1"?>
<!DOCTYPE rdf:RDF [
	<!ENTITY platform "http://localhost/~dennis/platformkit/2010_1/platform.owl#">
	<!ENTITY java "http://localhost/~dennis/platformkit/2010_1/java.owl#">
	<!ENTITY j2me-midp-1_0 "http://soft.vub.ac.be/platformkit/2010/1/j2me-midp-1_0.owl#">
	<!ENTITY isa "http://localhost/~dennis/platformkit/2010_1/isa.owl#">
	<!ENTITY xsd "http://www.w3.org/2001/XMLSchema#">
	<!ENTITY rdf "http://www.w3.org/1999/02/22-rdf-syntax-ns#">
	<!ENTITY owl "http://www.w3.org/2002/07/owl#">
	<!ENTITY ns_17 "http://localhost/~dennis/platformkit/2010_1/">
	<!ENTITY rdfs "http://www.w3.org/2000/01/rdf-schema#">
]>
<rdf:RDF
	 xmlns:platform="&platform;"
	 xmlns:java="&java;"
	 xmlns:j2me-midp-1_0="&j2me-midp-1_0;"
	 xmlns:isa="&isa;"
	 xmlns:xsd="&xsd;"
	 xmlns:rdf="&rdf;"
	 xmlns:owl="&owl;"
	 xmlns:ns_17="&ns_17;"
	 xmlns:rdfs="&rdfs;"
>

	<owl:Ontology rdf:about="http://soft.vub.ac.be/platformkit/2010/1/j2me-midp-1_0.owl#">
		<owl:versionInfo>$Id: UML2ToPackageAPIOntology.atl 8082 2010-03-18 21:11:00Z dwagelaa $</owl:versionInfo>
		<owl:imports rdf:resource="http://localhost/~dennis/platformkit/2010_1/platform.owl"/>
		<owl:imports rdf:resource="http://localhost/~dennis/platformkit/2010_1/java.owl"/>
		<rdfs:comment xml:lang="en">Generated by [UML2ToSimplifiedPackageAPIOntology.atl 8080 2010-03-18 10:46:40Z dwagelaa], [UML2ToPackageAPIOntology.atl 8082 2010-03-18 21:11:00Z dwagelaa], [UML2ToAPIOntology.atl 8082 2010-03-18 21:11:00Z dwagelaa], and [UML2Comparison.atl 8082 2010-03-18 21:11:00Z dwagelaa]</rdfs:comment>
		<rdfs:comment>Dennis Wagelaar &lt;dennis.wagelaar@vub.ac.be&gt;</rdfs:comment>
		<rdfs:comment xml:lang="en">&#169; 2010, Vrije Universiteit Brussel. All rights reserved.</rdfs:comment>
		<rdfs:label xml:lang="en">J2ME MIDP 1.0</rdfs:label>
	</owl:Ontology>
	<owl:Class rdf:about="&j2me-midp-1_0;J2MEMIDP1_0API">
		<rdfs:subClassOf rdf:resource="&j2me-midp-1_0;JavaLangAPI"/>
		<rdfs:subClassOf rdf:resource="&j2me-midp-1_0;JavaIoAPI"/>
		<rdfs:subClassOf rdf:resource="&j2me-midp-1_0;JavaUtilAPI"/>
		<rdfs:subClassOf rdf:resource="&j2me-midp-1_0;JavaxMicroeditionIoAPI"/>
		<rdfs:subClassOf rdf:resource="&j2me-midp-1_0;JavaxMicroeditionLcduiAPI"/>
		<rdfs:subClassOf rdf:resource="&j2me-midp-1_0;JavaxMicroeditionMidletAPI"/>
		<rdfs:subClassOf rdf:resource="&j2me-midp-1_0;JavaxMicroeditionRmsAPI"/>
		<rdfs:comment xml:lang="en">J2ME MIDP 1.0 API</rdfs:comment>
		<rdfs:comment xml:lang="OWLManchester">platform:comprisesInterfacePart some JavaLang and platform:comprisesInterfacePart some JavaIo and platform:comprisesInterfacePart some JavaUtil and platform:comprisesInterfacePart some JavaxMicroeditionIo and platform:comprisesInterfacePart some JavaxMicroeditionLcdui and platform:comprisesInterfacePart some JavaxMicroeditionMidlet and platform:comprisesInterfacePart some JavaxMicroeditionRms</rdfs:comment>
	</owl:Class>
	<owl:Class rdf:about="&j2me-midp-1_0;J2MEMIDP1_0ClassLibrary">
		<rdfs:subClassOf rdf:resource="&j2me-midp-1_0;JavaLangClassLibrary"/>
		<rdfs:subClassOf rdf:resource="&j2me-midp-1_0;JavaIoClassLibrary"/>
		<rdfs:subClassOf rdf:resource="&j2me-midp-1_0;JavaUtilClassLibrary"/>
		<rdfs:subClassOf rdf:resource="&j2me-midp-1_0;JavaxMicroeditionIoClassLibrary"/>
		<rdfs:subClassOf rdf:resource="&j2me-midp-1_0;JavaxMicroeditionLcduiClassLibrary"/>
		<rdfs:subClassOf rdf:resource="&j2me-midp-1_0;JavaxMicroeditionMidletClassLibrary"/>
		<rdfs:subClassOf rdf:resource="&j2me-midp-1_0;JavaxMicroeditionRmsClassLibrary"/>
		<rdfs:comment xml:lang="en">Java class library implementing the J2ME MIDP 1.0 API</rdfs:comment>
		<rdfs:comment xml:lang="OWLManchester">platform:implementsInterface some J2MEMIDP1_0API</rdfs:comment>
	</owl:Class>
	<owl:Class rdf:about="&j2me-midp-1_0;J2MEMIDP1_0BytecodeFormat">
		<rdfs:subClassOf rdf:resource="&isa;JavaBytecode"/>
		<rdfs:comment xml:lang="en">J2ME MIDP 1.0 bytecode format</rdfs:comment>
		<rdfs:comment xml:lang="OWLManchester">java:majorVersionNumber some xsd:integer[>="45"^^xsd:integer]</rdfs:comment>
	</owl:Class>
	<j2me-midp-1_0:J2MEMIDP1_0BytecodeFormat rdf:about="&j2me-midp-1_0;theJ2MEMIDP1_0BytecodeFormat">
		<java:preverified rdf:datatype="http://www.w3.org/2001/XMLSchema#boolean">true</java:preverified>
		<java:minorVersionNumber rdf:datatype="http://www.w3.org/2001/XMLSchema#integer">3</java:minorVersionNumber>
		<java:majorVersionNumber rdf:datatype="http://www.w3.org/2001/XMLSchema#integer">45</java:majorVersionNumber>
	</j2me-midp-1_0:J2MEMIDP1_0BytecodeFormat>
	<j2me-midp-1_0:J2MEMIDP1_0API rdf:about="&j2me-midp-1_0;theJ2MEMIDP1_0API">
		<platform:comprisesInterfacePart rdf:resource="&j2me-midp-1_0;theJavaxMicroeditionRmsPart"/>
		<platform:comprisesInterfacePart rdf:resource="&j2me-midp-1_0;theJavaxMicroeditionMidletPart"/>
		<platform:comprisesInterfacePart rdf:resource="&j2me-midp-1_0;theJavaxMicroeditionLcduiPart"/>
		<platform:comprisesInterfacePart rdf:resource="&j2me-midp-1_0;theJavaxMicroeditionIoPart"/>
		<platform:comprisesInterfacePart rdf:resource="&j2me-midp-1_0;theJavaUtilPart"/>
		<platform:comprisesInterfacePart rdf:resource="&j2me-midp-1_0;theJavaIoPart"/>
		<platform:comprisesInterfacePart rdf:resource="&j2me-midp-1_0;theJavaLangPart"/>
	</j2me-midp-1_0:J2MEMIDP1_0API>
	<owl:Class rdf:about="&j2me-midp-1_0;J2MEMIDP1_0VM">
		<owl:equivalentClass>
			<owl:Restriction>
				<owl:onProperty rdf:resource="&platform;implementsInterface"/>
				<owl:someValuesFrom rdf:resource="&j2me-midp-1_0;J2MEMIDP1_0BytecodeFormat"/>
			</owl:Restriction>
		</owl:equivalentClass>
		<rdfs:subClassOf rdf:resource="&java;JavaVM"/>
		<rdfs:comment xml:lang="en">J2ME MIDP 1.0 virtual machine</rdfs:comment>
	</owl:Class>
	<owl:Class rdf:about="&j2me-midp-1_0;J2MEMIDP1_0JRE">
		<owl:equivalentClass>
			<owl:Class >
				<owl:intersectionOf rdf:parseType="Collection">
					<owl:Restriction>
						<owl:onProperty rdf:resource="&platform;providesFeature"/>
						<owl:someValuesFrom rdf:resource="&j2me-midp-1_0;J2MEMIDP1_0ClassLibrary"/>
					</owl:Restriction>
					<owl:Restriction>
						<owl:onProperty rdf:resource="&platform;providesFeature"/>
						<owl:someValuesFrom rdf:resource="&j2me-midp-1_0;J2MEMIDP1_0VM"/>
					</owl:Restriction>
				</owl:intersectionOf>
			</owl:Class>
		</owl:equivalentClass>
		<rdfs:subClassOf rdf:resource="&java;JRE"/>
		<rdfs:comment xml:lang="en">J2ME MIDP 1.0 Java Runtime Environment</rdfs:comment>
	</owl:Class>
	<owl:Class rdf:about="&j2me-midp-1_0;JavaLang">
		<rdfs:subClassOf rdf:resource="&java;JavaAPIPart"/>
		<rdfs:seeAlso rdf:resource="&j2me-midp-1_0;JavaIo"/>
		<rdfs:comment xml:lang="en">Java API part implementing the java.lang package for J2ME MIDP 1.0</rdfs:comment>
	</owl:Class>
	<owl:Class rdf:about="&j2me-midp-1_0;JavaIo">
		<rdfs:subClassOf rdf:resource="&java;JavaAPIPart"/>
		<rdfs:seeAlso rdf:resource="&j2me-midp-1_0;JavaLang"/>
		<rdfs:comment xml:lang="en">Java API part implementing the java.io package for J2ME MIDP 1.0</rdfs:comment>
	</owl:Class>
	<owl:Class rdf:about="&j2me-midp-1_0;JavaUtil">
		<rdfs:subClassOf rdf:resource="&java;JavaAPIPart"/>
		<rdfs:seeAlso rdf:resource="&j2me-midp-1_0;JavaLang"/>
		<rdfs:comment xml:lang="en">Java API part implementing the java.util package for J2ME MIDP 1.0</rdfs:comment>
	</owl:Class>
	<owl:Class rdf:about="&j2me-midp-1_0;JavaxMicroeditionIo">
		<rdfs:subClassOf rdf:resource="&java;JavaAPIPart"/>
		<rdfs:seeAlso rdf:resource="&j2me-midp-1_0;JavaLang"/>
		<rdfs:seeAlso rdf:resource="&j2me-midp-1_0;JavaIo"/>
		<rdfs:comment xml:lang="en">Java API part implementing the javax.microedition.io package for J2ME MIDP 1.0</rdfs:comment>
	</owl:Class>
	<owl:Class rdf:about="&j2me-midp-1_0;JavaxMicroeditionLcdui">
		<rdfs:subClassOf rdf:resource="&java;JavaAPIPart"/>
		<rdfs:seeAlso rdf:resource="&j2me-midp-1_0;JavaLang"/>
		<rdfs:seeAlso rdf:resource="&j2me-midp-1_0;JavaxMicroeditionMidlet"/>
		<rdfs:seeAlso rdf:resource="&j2me-midp-1_0;JavaUtil"/>
		<rdfs:comment xml:lang="en">Java API part implementing the javax.microedition.lcdui package for J2ME MIDP 1.0</rdfs:comment>
	</owl:Class>
	<owl:Class rdf:about="&j2me-midp-1_0;JavaxMicroeditionMidlet">
		<rdfs:subClassOf rdf:resource="&java;JavaAPIPart"/>
		<rdfs:seeAlso rdf:resource="&j2me-midp-1_0;JavaLang"/>
		<rdfs:comment xml:lang="en">Java API part implementing the javax.microedition.midlet package for J2ME MIDP 1.0</rdfs:comment>
	</owl:Class>
	<owl:Class rdf:about="&j2me-midp-1_0;JavaxMicroeditionRms">
		<rdfs:subClassOf rdf:resource="&java;JavaAPIPart"/>
		<rdfs:seeAlso rdf:resource="&j2me-midp-1_0;JavaLang"/>
		<rdfs:comment xml:lang="en">Java API part implementing the javax.microedition.rms package for J2ME MIDP 1.0</rdfs:comment>
	</owl:Class>
	<owl:Class rdf:about="&j2me-midp-1_0;JavaLangAPI">
		<rdfs:subClassOf rdf:resource="&java;JavaAPI"/>
		<rdfs:comment xml:lang="en">JavaLibrary implementing the java.lang package for J2ME MIDP 1.0</rdfs:comment>
		<rdfs:comment xml:lang="OWLManchester">platform:comprisesInterfacePart some JavaLang</rdfs:comment>
	</owl:Class>
	<owl:Class rdf:about="&j2me-midp-1_0;JavaIoAPI">
		<rdfs:subClassOf rdf:resource="&java;JavaAPI"/>
		<rdfs:comment xml:lang="en">JavaLibrary implementing the java.io package for J2ME MIDP 1.0</rdfs:comment>
		<rdfs:comment xml:lang="OWLManchester">platform:comprisesInterfacePart some JavaIo</rdfs:comment>
	</owl:Class>
	<owl:Class rdf:about="&j2me-midp-1_0;JavaUtilAPI">
		<rdfs:subClassOf rdf:resource="&java;JavaAPI"/>
		<rdfs:comment xml:lang="en">JavaLibrary implementing the java.util package for J2ME MIDP 1.0</rdfs:comment>
		<rdfs:comment xml:lang="OWLManchester">platform:comprisesInterfacePart some JavaUtil</rdfs:comment>
	</owl:Class>
	<owl:Class rdf:about="&j2me-midp-1_0;JavaxMicroeditionIoAPI">
		<rdfs:subClassOf rdf:resource="&java;JavaAPI"/>
		<rdfs:comment xml:lang="en">JavaLibrary implementing the javax.microedition.io package for J2ME MIDP 1.0</rdfs:comment>
		<rdfs:comment xml:lang="OWLManchester">platform:comprisesInterfacePart some JavaxMicroeditionIo</rdfs:comment>
	</owl:Class>
	<owl:Class rdf:about="&j2me-midp-1_0;JavaxMicroeditionLcduiAPI">
		<rdfs:subClassOf rdf:resource="&java;JavaAPI"/>
		<rdfs:comment xml:lang="en">JavaLibrary implementing the javax.microedition.lcdui package for J2ME MIDP 1.0</rdfs:comment>
		<rdfs:comment xml:lang="OWLManchester">platform:comprisesInterfacePart some JavaxMicroeditionLcdui</rdfs:comment>
	</owl:Class>
	<owl:Class rdf:about="&j2me-midp-1_0;JavaxMicroeditionMidletAPI">
		<rdfs:subClassOf rdf:resource="&java;JavaAPI"/>
		<rdfs:comment xml:lang="en">JavaLibrary implementing the javax.microedition.midlet package for J2ME MIDP 1.0</rdfs:comment>
		<rdfs:comment xml:lang="OWLManchester">platform:comprisesInterfacePart some JavaxMicroeditionMidlet</rdfs:comment>
	</owl:Class>
	<owl:Class rdf:about="&j2me-midp-1_0;JavaxMicroeditionRmsAPI">
		<rdfs:subClassOf rdf:resource="&java;JavaAPI"/>
		<rdfs:comment xml:lang="en">JavaLibrary implementing the javax.microedition.rms package for J2ME MIDP 1.0</rdfs:comment>
		<rdfs:comment xml:lang="OWLManchester">platform:comprisesInterfacePart some JavaxMicroeditionRms</rdfs:comment>
	</owl:Class>
	<j2me-midp-1_0:JavaLang rdf:about="&j2me-midp-1_0;theJavaLangPart">
	</j2me-midp-1_0:JavaLang>
	<j2me-midp-1_0:JavaIo rdf:about="&j2me-midp-1_0;theJavaIoPart">
	</j2me-midp-1_0:JavaIo>
	<j2me-midp-1_0:JavaUtil rdf:about="&j2me-midp-1_0;theJavaUtilPart">
	</j2me-midp-1_0:JavaUtil>
	<j2me-midp-1_0:JavaxMicroeditionIo rdf:about="&j2me-midp-1_0;theJavaxMicroeditionIoPart">
	</j2me-midp-1_0:JavaxMicroeditionIo>
	<j2me-midp-1_0:JavaxMicroeditionLcdui rdf:about="&j2me-midp-1_0;theJavaxMicroeditionLcduiPart">
	</j2me-midp-1_0:JavaxMicroeditionLcdui>
	<j2me-midp-1_0:JavaxMicroeditionMidlet rdf:about="&j2me-midp-1_0;theJavaxMicroeditionMidletPart">
	</j2me-midp-1_0:JavaxMicroeditionMidlet>
	<j2me-midp-1_0:JavaxMicroeditionRms rdf:about="&j2me-midp-1_0;theJavaxMicroeditionRmsPart">
	</j2me-midp-1_0:JavaxMicroeditionRms>
	<owl:Class rdf:about="&j2me-midp-1_0;JavaLangClassLibrary">
		<rdfs:subClassOf rdf:resource="&java;JavaClassLibrary"/>
		<rdfs:comment xml:lang="en">JavaLibrary implementing the java.lang package for J2ME MIDP 1.0</rdfs:comment>
		<rdfs:comment xml:lang="OWLManchester">platform:implementsInterface some JavaLangAPI</rdfs:comment>
	</owl:Class>
	<owl:Class rdf:about="&j2me-midp-1_0;JavaIoClassLibrary">
		<rdfs:subClassOf rdf:resource="&java;JavaClassLibrary"/>
		<rdfs:comment xml:lang="en">JavaLibrary implementing the java.io package for J2ME MIDP 1.0</rdfs:comment>
		<rdfs:comment xml:lang="OWLManchester">platform:implementsInterface some JavaIoAPI</rdfs:comment>
	</owl:Class>
	<owl:Class rdf:about="&j2me-midp-1_0;JavaUtilClassLibrary">
		<rdfs:subClassOf rdf:resource="&java;JavaClassLibrary"/>
		<rdfs:comment xml:lang="en">JavaLibrary implementing the java.util package for J2ME MIDP 1.0</rdfs:comment>
		<rdfs:comment xml:lang="OWLManchester">platform:implementsInterface some JavaUtilAPI</rdfs:comment>
	</owl:Class>
	<owl:Class rdf:about="&j2me-midp-1_0;JavaxMicroeditionIoClassLibrary">
		<rdfs:subClassOf rdf:resource="&java;JavaClassLibrary"/>
		<rdfs:comment xml:lang="en">JavaLibrary implementing the javax.microedition.io package for J2ME MIDP 1.0</rdfs:comment>
		<rdfs:comment xml:lang="OWLManchester">platform:implementsInterface some JavaxMicroeditionIoAPI</rdfs:comment>
	</owl:Class>
	<owl:Class rdf:about="&j2me-midp-1_0;JavaxMicroeditionLcduiClassLibrary">
		<rdfs:subClassOf rdf:resource="&java;JavaClassLibrary"/>
		<rdfs:comment xml:lang="en">JavaLibrary implementing the javax.microedition.lcdui package for J2ME MIDP 1.0</rdfs:comment>
		<rdfs:comment xml:lang="OWLManchester">platform:implementsInterface some JavaxMicroeditionLcduiAPI</rdfs:comment>
	</owl:Class>
	<owl:Class rdf:about="&j2me-midp-1_0;JavaxMicroeditionMidletClassLibrary">
		<rdfs:subClassOf rdf:resource="&java;JavaClassLibrary"/>
		<rdfs:comment xml:lang="en">JavaLibrary implementing the javax.microedition.midlet package for J2ME MIDP 1.0</rdfs:comment>
		<rdfs:comment xml:lang="OWLManchester">platform:implementsInterface some JavaxMicroeditionMidletAPI</rdfs:comment>
	</owl:Class>
	<owl:Class rdf:about="&j2me-midp-1_0;JavaxMicroeditionRmsClassLibrary">
		<rdfs:subClassOf rdf:resource="&java;JavaClassLibrary"/>
		<rdfs:comment xml:lang="en">JavaLibrary implementing the javax.microedition.rms package for J2ME MIDP 1.0</rdfs:comment>
		<rdfs:comment xml:lang="OWLManchester">platform:implementsInterface some JavaxMicroeditionRmsAPI</rdfs:comment>
	</owl:Class>
</rdf:RDF>
