<?xml version="1.0" encoding="ISO-8859-1"?>
<!DOCTYPE rdf:RDF [
	<!ENTITY xsd "http://www.w3.org/2001/XMLSchema#">
	<!ENTITY java "http://localhost/~dennis/platformkit/2010_1/java.owl#">
	<!ENTITY ns_19 "http://localhost/~dennis/platformkit/2010_1/">
	<!ENTITY j2se-1_4 "http://soft.vub.ac.be/platformkit/2010/1/j2se-1_4.owl#">
	<!ENTITY j2me-pp-1_1 "http://soft.vub.ac.be/platformkit/2010/1/j2me-pp-1_1.owl#">
	<!ENTITY isa "http://localhost/~dennis/platformkit/2010_1/isa.owl#">
	<!ENTITY platform "http://localhost/~dennis/platformkit/2010_1/platform.owl#">
	<!ENTITY j2se-1_3 "http://soft.vub.ac.be/platformkit/2010/1/j2se-1_3.owl#">
	<!ENTITY rdf "http://www.w3.org/1999/02/22-rdf-syntax-ns#">
	<!ENTITY rdfs "http://www.w3.org/2000/01/rdf-schema#">
	<!ENTITY owl "http://www.w3.org/2002/07/owl#">
]>
<rdf:RDF
	 xmlns:xsd="&xsd;"
	 xmlns:java="&java;"
	 xmlns:ns_19="&ns_19;"
	 xmlns:j2se-1_4="&j2se-1_4;"
	 xmlns:j2me-pp-1_1="&j2me-pp-1_1;"
	 xmlns:isa="&isa;"
	 xmlns:platform="&platform;"
	 xmlns:j2se-1_3="&j2se-1_3;"
	 xmlns:rdf="&rdf;"
	 xmlns:rdfs="&rdfs;"
	 xmlns:owl="&owl;"
>

	<owl:Ontology rdf:about="http://soft.vub.ac.be/platformkit/2010/1/j2se-1_4.owl#">
		<owl:versionInfo>$Id: UML2ToPackageAPIOntology.atl 8082 2010-03-18 21:11:00Z dwagelaa $</owl:versionInfo>
		<owl:imports rdf:resource="http://localhost/~dennis/platformkit/2010_1/platform.owl"/>
		<owl:imports rdf:resource="http://localhost/~dennis/platformkit/2010_1/java.owl"/>
		<owl:imports rdf:resource="http://soft.vub.ac.be/platformkit/2010/1/j2se-1_3.owl#"/>
		<owl:imports rdf:resource="http://localhost/~dennis/platformkit/2010_1/isa.owl"/>
		<owl:imports rdf:resource="http://soft.vub.ac.be/platformkit/2010/1/j2me-pp-1_1.owl#"/>
		<rdfs:comment xml:lang="en">Generated by [UML2ToSimplifiedPackageAPIOntology.atl 8080 2010-03-18 10:46:40Z dwagelaa], [UML2ToPackageAPIOntology.atl 8082 2010-03-18 21:11:00Z dwagelaa], [UML2ToAPIOntology.atl 8082 2010-03-18 21:11:00Z dwagelaa], and [UML2Comparison.atl 8082 2010-03-18 21:11:00Z dwagelaa]</rdfs:comment>
		<rdfs:comment>Dennis Wagelaar &lt;dennis.wagelaar@vub.ac.be&gt;</rdfs:comment>
		<rdfs:comment xml:lang="en">&#169; 2010, Vrije Universiteit Brussel. All rights reserved.</rdfs:comment>
		<rdfs:label xml:lang="en">J2SE 1.4</rdfs:label>
	</owl:Ontology>
	<owl:Class rdf:about="&j2se-1_4;J2SE1_4API">
		<rdfs:subClassOf rdf:resource="&j2se-1_4;JavaLangAPI"/>
		<rdfs:subClassOf rdf:resource="&j2se-1_4;JavaLangReflectAPI"/>
		<rdfs:subClassOf rdf:resource="&j2se-1_4;JavaLangRefAPI"/>
		<rdfs:subClassOf rdf:resource="&j2se-1_4;JavaIoAPI"/>
		<rdfs:subClassOf rdf:resource="&j2se-1_4;JavaUtilAPI"/>
		<rdfs:subClassOf rdf:resource="&j2se-1_4;JavaUtilLoggingAPI"/>
		<rdfs:subClassOf rdf:resource="&j2se-1_4;JavaUtilJarAPI"/>
		<rdfs:subClassOf rdf:resource="&j2se-1_4;JavaUtilZipAPI"/>
		<rdfs:subClassOf rdf:resource="&j2se-1_4;JavaUtilPrefsAPI"/>
		<rdfs:subClassOf rdf:resource="&j2se-1_4;JavaUtilRegexAPI"/>
		<rdfs:subClassOf rdf:resource="&j2se-1_4;JavaNetAPI"/>
		<rdfs:subClassOf rdf:resource="&j2se-1_4;JavaSecurityAPI"/>
		<rdfs:subClassOf rdf:resource="&j2se-1_4;JavaSecurityCertAPI"/>
		<rdfs:subClassOf rdf:resource="&j2se-1_4;JavaSecuritySpecAPI"/>
		<rdfs:subClassOf rdf:resource="&j2se-1_4;JavaSecurityAclAPI"/>
		<rdfs:subClassOf rdf:resource="&j2se-1_4;JavaSecurityInterfacesAPI"/>
		<rdfs:subClassOf rdf:resource="&j2se-1_4;JavaNioAPI"/>
		<rdfs:subClassOf rdf:resource="&j2se-1_4;JavaNioChannelsAPI"/>
		<rdfs:subClassOf rdf:resource="&j2se-1_4;JavaNioChannelsSpiAPI"/>
		<rdfs:subClassOf rdf:resource="&j2se-1_4;JavaNioCharsetAPI"/>
		<rdfs:subClassOf rdf:resource="&j2se-1_4;JavaNioCharsetSpiAPI"/>
		<rdfs:subClassOf rdf:resource="&j2se-1_4;JavaBeansAPI"/>
		<rdfs:subClassOf rdf:resource="&j2se-1_4;JavaBeansBeancontextAPI"/>
		<rdfs:subClassOf rdf:resource="&j2se-1_4;JavaAwtAPI"/>
		<rdfs:subClassOf rdf:resource="&j2se-1_4;JavaAwtImageAPI"/>
		<rdfs:subClassOf rdf:resource="&j2se-1_4;JavaAwtImageRenderableAPI"/>
		<rdfs:subClassOf rdf:resource="&j2se-1_4;JavaAwtDatatransferAPI"/>
		<rdfs:subClassOf rdf:resource="&j2se-1_4;JavaAwtDndAPI"/>
		<rdfs:subClassOf rdf:resource="&j2se-1_4;JavaAwtEventAPI"/>
		<rdfs:subClassOf rdf:resource="&j2se-1_4;JavaAwtImAPI"/>
		<rdfs:subClassOf rdf:resource="&j2se-1_4;JavaAwtImSpiAPI"/>
		<rdfs:subClassOf rdf:resource="&j2se-1_4;JavaAwtFontAPI"/>
		<rdfs:subClassOf rdf:resource="&j2se-1_4;JavaAwtGeomAPI"/>
		<rdfs:subClassOf rdf:resource="&j2se-1_4;JavaAwtColorAPI"/>
		<rdfs:subClassOf rdf:resource="&j2se-1_4;JavaAwtPrintAPI"/>
		<rdfs:subClassOf rdf:resource="&j2se-1_4;JavaTextAPI"/>
		<rdfs:subClassOf rdf:resource="&j2se-1_4;JavaMathAPI"/>
		<rdfs:subClassOf rdf:resource="&j2se-1_4;JavaAppletAPI"/>
		<rdfs:subClassOf rdf:resource="&j2se-1_4;JavaRmiAPI"/>
		<rdfs:subClassOf rdf:resource="&j2se-1_4;JavaRmiActivationAPI"/>
		<rdfs:subClassOf rdf:resource="&j2se-1_4;JavaRmiServerAPI"/>
		<rdfs:subClassOf rdf:resource="&j2se-1_4;JavaRmiDgcAPI"/>
		<rdfs:subClassOf rdf:resource="&j2se-1_4;JavaRmiRegistryAPI"/>
		<rdfs:subClassOf rdf:resource="&j2se-1_4;JavaSqlAPI"/>
		<rdfs:subClassOf rdf:resource="&j2se-1_4;JavaxImageioAPI"/>
		<rdfs:subClassOf rdf:resource="&j2se-1_4;JavaxImageioSpiAPI"/>
		<rdfs:subClassOf rdf:resource="&j2se-1_4;JavaxImageioMetadataAPI"/>
		<rdfs:subClassOf rdf:resource="&j2se-1_4;JavaxImageioStreamAPI"/>
		<rdfs:subClassOf rdf:resource="&j2se-1_4;JavaxImageioEventAPI"/>
		<rdfs:subClassOf rdf:resource="&j2se-1_4;JavaxImageioPluginsJpegAPI"/>
		<rdfs:subClassOf rdf:resource="&j2se-1_4;JavaxAccessibilityAPI"/>
		<rdfs:subClassOf rdf:resource="&j2se-1_4;JavaxSwingAPI"/>
		<rdfs:subClassOf rdf:resource="&j2se-1_4;JavaxSwingPlafAPI"/>
		<rdfs:subClassOf rdf:resource="&j2se-1_4;JavaxSwingPlafBasicAPI"/>
		<rdfs:subClassOf rdf:resource="&j2se-1_4;JavaxSwingPlafMetalAPI"/>
		<rdfs:subClassOf rdf:resource="&j2se-1_4;JavaxSwingPlafMultiAPI"/>
		<rdfs:subClassOf rdf:resource="&j2se-1_4;JavaxSwingEventAPI"/>
		<rdfs:subClassOf rdf:resource="&j2se-1_4;JavaxSwingBorderAPI"/>
		<rdfs:subClassOf rdf:resource="&j2se-1_4;JavaxSwingTextAPI"/>
		<rdfs:subClassOf rdf:resource="&j2se-1_4;JavaxSwingTextHtmlAPI"/>
		<rdfs:subClassOf rdf:resource="&j2se-1_4;JavaxSwingTextHtmlParserAPI"/>
		<rdfs:subClassOf rdf:resource="&j2se-1_4;JavaxSwingTextRtfAPI"/>
		<rdfs:subClassOf rdf:resource="&j2se-1_4;JavaxSwingTableAPI"/>
		<rdfs:subClassOf rdf:resource="&j2se-1_4;JavaxSwingUndoAPI"/>
		<rdfs:subClassOf rdf:resource="&j2se-1_4;JavaxSwingTreeAPI"/>
		<rdfs:subClassOf rdf:resource="&j2se-1_4;JavaxSwingFilechooserAPI"/>
		<rdfs:subClassOf rdf:resource="&j2se-1_4;JavaxSwingColorchooserAPI"/>
		<rdfs:subClassOf rdf:resource="&j2se-1_4;JavaxSoundSampledAPI"/>
		<rdfs:subClassOf rdf:resource="&j2se-1_4;JavaxSoundSampledSpiAPI"/>
		<rdfs:subClassOf rdf:resource="&j2se-1_4;JavaxSoundMidiAPI"/>
		<rdfs:subClassOf rdf:resource="&j2se-1_4;JavaxSoundMidiSpiAPI"/>
		<rdfs:subClassOf rdf:resource="&j2se-1_4;JavaxPrintAPI"/>
		<rdfs:subClassOf rdf:resource="&j2se-1_4;JavaxPrintAttributeAPI"/>
		<rdfs:subClassOf rdf:resource="&j2se-1_4;JavaxPrintAttributeStandardAPI"/>
		<rdfs:subClassOf rdf:resource="&j2se-1_4;JavaxPrintEventAPI"/>
		<rdfs:subClassOf rdf:resource="&j2se-1_4;JavaxSecurityAuthAPI"/>
		<rdfs:subClassOf rdf:resource="&j2se-1_4;JavaxSecurityAuthX500API"/>
		<rdfs:subClassOf rdf:resource="&j2se-1_4;JavaxSecurityAuthCallbackAPI"/>
		<rdfs:subClassOf rdf:resource="&j2se-1_4;JavaxSecurityAuthKerberosAPI"/>
		<rdfs:subClassOf rdf:resource="&j2se-1_4;JavaxSecurityAuthLoginAPI"/>
		<rdfs:subClassOf rdf:resource="&j2se-1_4;JavaxSecurityAuthSpiAPI"/>
		<rdfs:subClassOf rdf:resource="&j2se-1_4;JavaxSecurityCertAPI"/>
		<rdfs:subClassOf rdf:resource="&j2se-1_4;JavaxNamingAPI"/>
		<rdfs:subClassOf rdf:resource="&j2se-1_4;JavaxNamingDirectoryAPI"/>
		<rdfs:subClassOf rdf:resource="&j2se-1_4;JavaxNamingEventAPI"/>
		<rdfs:subClassOf rdf:resource="&j2se-1_4;JavaxNamingLdapAPI"/>
		<rdfs:subClassOf rdf:resource="&j2se-1_4;JavaxNamingSpiAPI"/>
		<rdfs:subClassOf rdf:resource="&j2se-1_4;JavaxNetAPI"/>
		<rdfs:subClassOf rdf:resource="&j2se-1_4;JavaxNetSslAPI"/>
		<rdfs:subClassOf rdf:resource="&j2se-1_4;JavaxRmiAPI"/>
		<rdfs:subClassOf rdf:resource="&j2se-1_4;JavaxRmiCORBAAPI"/>
		<rdfs:subClassOf rdf:resource="&j2se-1_4;JavaxCryptoAPI"/>
		<rdfs:subClassOf rdf:resource="&j2se-1_4;JavaxCryptoInterfacesAPI"/>
		<rdfs:subClassOf rdf:resource="&j2se-1_4;JavaxCryptoSpecAPI"/>
		<rdfs:subClassOf rdf:resource="&j2se-1_4;JavaxSqlAPI"/>
		<rdfs:subClassOf rdf:resource="&j2se-1_4;JavaxTransactionAPI"/>
		<rdfs:subClassOf rdf:resource="&j2se-1_4;JavaxTransactionXaAPI"/>
		<rdfs:subClassOf rdf:resource="&j2se-1_4;JavaxXmlParsersAPI"/>
		<rdfs:subClassOf rdf:resource="&j2se-1_4;JavaxXmlTransformAPI"/>
		<rdfs:subClassOf rdf:resource="&j2se-1_4;JavaxXmlTransformDomAPI"/>
		<rdfs:subClassOf rdf:resource="&j2se-1_4;JavaxXmlTransformSaxAPI"/>
		<rdfs:subClassOf rdf:resource="&j2se-1_4;JavaxXmlTransformStreamAPI"/>
		<rdfs:subClassOf rdf:resource="&j2se-1_4;OrgW3cDomAPI"/>
		<rdfs:subClassOf rdf:resource="&j2se-1_4;OrgW3cDomCssAPI"/>
		<rdfs:subClassOf rdf:resource="&j2se-1_4;OrgW3cDomStylesheetsAPI"/>
		<rdfs:subClassOf rdf:resource="&j2se-1_4;OrgW3cDomViewsAPI"/>
		<rdfs:subClassOf rdf:resource="&j2se-1_4;OrgW3cDomEventsAPI"/>
		<rdfs:subClassOf rdf:resource="&j2se-1_4;OrgW3cDomHtmlAPI"/>
		<rdfs:subClassOf rdf:resource="&j2se-1_4;OrgW3cDomTraversalAPI"/>
		<rdfs:subClassOf rdf:resource="&j2se-1_4;OrgOmgCORBA_2_3API"/>
		<rdfs:subClassOf rdf:resource="&j2se-1_4;OrgOmgCORBA_2_3PortableAPI"/>
		<rdfs:subClassOf rdf:resource="&j2se-1_4;OrgOmgCORBAAPI"/>
		<rdfs:subClassOf rdf:resource="&j2se-1_4;OrgOmgCORBAPortableAPI"/>
		<rdfs:subClassOf rdf:resource="&j2se-1_4;OrgOmgCORBADynAnyPackageAPI"/>
		<rdfs:subClassOf rdf:resource="&j2se-1_4;OrgOmgCORBAORBPackageAPI"/>
		<rdfs:subClassOf rdf:resource="&j2se-1_4;OrgOmgCORBATypeCodePackageAPI"/>
		<rdfs:subClassOf rdf:resource="&j2se-1_4;OrgOmgSendingContextAPI"/>
		<rdfs:subClassOf rdf:resource="&j2se-1_4;OrgOmgCosNamingAPI"/>
		<rdfs:subClassOf rdf:resource="&j2se-1_4;OrgOmgCosNamingNamingContextExtPackageAPI"/>
		<rdfs:subClassOf rdf:resource="&j2se-1_4;OrgOmgCosNamingNamingContextPackageAPI"/>
		<rdfs:subClassOf rdf:resource="&j2se-1_4;OrgOmgPortableServerAPI"/>
		<rdfs:subClassOf rdf:resource="&j2se-1_4;OrgOmgPortableServerCurrentPackageAPI"/>
		<rdfs:subClassOf rdf:resource="&j2se-1_4;OrgOmgPortableServerPOAManagerPackageAPI"/>
		<rdfs:subClassOf rdf:resource="&j2se-1_4;OrgOmgPortableServerPOAPackageAPI"/>
		<rdfs:subClassOf rdf:resource="&j2se-1_4;OrgOmgPortableServerPortableAPI"/>
		<rdfs:subClassOf rdf:resource="&j2se-1_4;OrgOmgPortableServerServantLocatorPackageAPI"/>
		<rdfs:subClassOf rdf:resource="&j2se-1_4;OrgOmgDynamicAPI"/>
		<rdfs:subClassOf rdf:resource="&j2se-1_4;OrgOmgDynamicAnyAPI"/>
		<rdfs:subClassOf rdf:resource="&j2se-1_4;OrgOmgDynamicAnyDynAnyFactoryPackageAPI"/>
		<rdfs:subClassOf rdf:resource="&j2se-1_4;OrgOmgDynamicAnyDynAnyPackageAPI"/>
		<rdfs:subClassOf rdf:resource="&j2se-1_4;OrgOmgIOPAPI"/>
		<rdfs:subClassOf rdf:resource="&j2se-1_4;OrgOmgIOPCodecFactoryPackageAPI"/>
		<rdfs:subClassOf rdf:resource="&j2se-1_4;OrgOmgIOPCodecPackageAPI"/>
		<rdfs:subClassOf rdf:resource="&j2se-1_4;OrgOmgMessagingAPI"/>
		<rdfs:subClassOf rdf:resource="&j2se-1_4;OrgOmgPortableInterceptorAPI"/>
		<rdfs:subClassOf rdf:resource="&j2se-1_4;OrgOmgPortableInterceptorORBInitInfoPackageAPI"/>
		<rdfs:subClassOf rdf:resource="&j2se-1_4;OrgOmgStubJavaRmiAPI"/>
		<rdfs:subClassOf rdf:resource="&j2se-1_4;OrgXmlSaxAPI"/>
		<rdfs:subClassOf rdf:resource="&j2se-1_4;OrgXmlSaxHelpersAPI"/>
		<rdfs:subClassOf rdf:resource="&j2se-1_4;OrgXmlSaxExtAPI"/>
		<rdfs:subClassOf rdf:resource="&j2se-1_4;OrgIetfJgssAPI"/>
		<rdfs:comment xml:lang="en">J2SE 1.4 API</rdfs:comment>
		<rdfs:comment xml:lang="OWLManchester">platform:comprisesInterfacePart some JavaLang and platform:comprisesInterfacePart some JavaLangReflect and platform:comprisesInterfacePart some JavaLangRef and platform:comprisesInterfacePart some JavaIo and platform:comprisesInterfacePart some JavaUtil and platform:comprisesInterfacePart some JavaUtilLogging and platform:comprisesInterfacePart some JavaUtilJar and platform:comprisesInterfacePart some JavaUtilZip and platform:comprisesInterfacePart some JavaUtilPrefs and platform:comprisesInterfacePart some JavaUtilRegex and platform:comprisesInterfacePart some JavaNet and platform:comprisesInterfacePart some JavaSecurity and platform:comprisesInterfacePart some JavaSecurityCert and platform:comprisesInterfacePart some JavaSecuritySpec and platform:comprisesInterfacePart some JavaSecurityAcl and platform:comprisesInterfacePart some JavaSecurityInterfaces and platform:comprisesInterfacePart some JavaNio and platform:comprisesInterfacePart some JavaNioChannels and platform:comprisesInterfacePart some JavaNioChannelsSpi and platform:comprisesInterfacePart some JavaNioCharset and platform:comprisesInterfacePart some JavaNioCharsetSpi and platform:comprisesInterfacePart some JavaBeans and platform:comprisesInterfacePart some JavaBeansBeancontext and platform:comprisesInterfacePart some JavaAwt and platform:comprisesInterfacePart some JavaAwtImage and platform:comprisesInterfacePart some JavaAwtImageRenderable and platform:comprisesInterfacePart some JavaAwtDatatransfer and platform:comprisesInterfacePart some JavaAwtDnd and platform:comprisesInterfacePart some JavaAwtEvent and platform:comprisesInterfacePart some JavaAwtIm and platform:comprisesInterfacePart some JavaAwtImSpi and platform:comprisesInterfacePart some JavaAwtFont and platform:comprisesInterfacePart some JavaAwtGeom and platform:comprisesInterfacePart some JavaAwtColor and platform:comprisesInterfacePart some JavaAwtPrint and platform:comprisesInterfacePart some JavaText and platform:comprisesInterfacePart some JavaMath and platform:comprisesInterfacePart some JavaApplet and platform:comprisesInterfacePart some JavaRmi and platform:comprisesInterfacePart some JavaRmiActivation and platform:comprisesInterfacePart some JavaRmiServer and platform:comprisesInterfacePart some JavaRmiDgc and platform:comprisesInterfacePart some JavaRmiRegistry and platform:comprisesInterfacePart some JavaSql and platform:comprisesInterfacePart some JavaxImageio and platform:comprisesInterfacePart some JavaxImageioSpi and platform:comprisesInterfacePart some JavaxImageioMetadata and platform:comprisesInterfacePart some JavaxImageioStream and platform:comprisesInterfacePart some JavaxImageioEvent and platform:comprisesInterfacePart some JavaxImageioPluginsJpeg and platform:comprisesInterfacePart some JavaxAccessibility and platform:comprisesInterfacePart some JavaxSwing and platform:comprisesInterfacePart some JavaxSwingPlaf and platform:comprisesInterfacePart some JavaxSwingPlafBasic and platform:comprisesInterfacePart some JavaxSwingPlafMetal and platform:comprisesInterfacePart some JavaxSwingPlafMulti and platform:comprisesInterfacePart some JavaxSwingEvent and platform:comprisesInterfacePart some JavaxSwingBorder and platform:comprisesInterfacePart some JavaxSwingText and platform:comprisesInterfacePart some JavaxSwingTextHtml and platform:comprisesInterfacePart some JavaxSwingTextHtmlParser and platform:comprisesInterfacePart some JavaxSwingTextRtf and platform:comprisesInterfacePart some JavaxSwingTable and platform:comprisesInterfacePart some JavaxSwingUndo and platform:comprisesInterfacePart some JavaxSwingTree and platform:comprisesInterfacePart some JavaxSwingFilechooser and platform:comprisesInterfacePart some JavaxSwingColorchooser and platform:comprisesInterfacePart some JavaxSoundSampled and platform:comprisesInterfacePart some JavaxSoundSampledSpi and platform:comprisesInterfacePart some JavaxSoundMidi and platform:comprisesInterfacePart some JavaxSoundMidiSpi and platform:comprisesInterfacePart some JavaxPrint and platform:comprisesInterfacePart some JavaxPrintAttribute and platform:comprisesInterfacePart some JavaxPrintAttributeStandard and platform:comprisesInterfacePart some JavaxPrintEvent and platform:comprisesInterfacePart some JavaxSecurityAuth and platform:comprisesInterfacePart some JavaxSecurityAuthX500 and platform:comprisesInterfacePart some JavaxSecurityAuthCallback and platform:comprisesInterfacePart some JavaxSecurityAuthKerberos and platform:comprisesInterfacePart some JavaxSecurityAuthLogin and platform:comprisesInterfacePart some JavaxSecurityAuthSpi and platform:comprisesInterfacePart some JavaxSecurityCert and platform:comprisesInterfacePart some JavaxNaming and platform:comprisesInterfacePart some JavaxNamingDirectory and platform:comprisesInterfacePart some JavaxNamingEvent and platform:comprisesInterfacePart some JavaxNamingLdap and platform:comprisesInterfacePart some JavaxNamingSpi and platform:comprisesInterfacePart some JavaxNet and platform:comprisesInterfacePart some JavaxNetSsl and platform:comprisesInterfacePart some JavaxRmi and platform:comprisesInterfacePart some JavaxRmiCORBA and platform:comprisesInterfacePart some JavaxCrypto and platform:comprisesInterfacePart some JavaxCryptoInterfaces and platform:comprisesInterfacePart some JavaxCryptoSpec and platform:comprisesInterfacePart some JavaxSql and platform:comprisesInterfacePart some JavaxTransaction and platform:comprisesInterfacePart some JavaxTransactionXa and platform:comprisesInterfacePart some JavaxXmlParsers and platform:comprisesInterfacePart some JavaxXmlTransform and platform:comprisesInterfacePart some JavaxXmlTransformDom and platform:comprisesInterfacePart some JavaxXmlTransformSax and platform:comprisesInterfacePart some JavaxXmlTransformStream and platform:comprisesInterfacePart some OrgW3cDom and platform:comprisesInterfacePart some OrgW3cDomCss and platform:comprisesInterfacePart some OrgW3cDomStylesheets and platform:comprisesInterfacePart some OrgW3cDomViews and platform:comprisesInterfacePart some OrgW3cDomEvents and platform:comprisesInterfacePart some OrgW3cDomHtml and platform:comprisesInterfacePart some OrgW3cDomTraversal and platform:comprisesInterfacePart some OrgOmgCORBA_2_3 and platform:comprisesInterfacePart some OrgOmgCORBA_2_3Portable and platform:comprisesInterfacePart some OrgOmgCORBA and platform:comprisesInterfacePart some OrgOmgCORBAPortable and platform:comprisesInterfacePart some OrgOmgCORBADynAnyPackage and platform:comprisesInterfacePart some OrgOmgCORBAORBPackage and platform:comprisesInterfacePart some OrgOmgCORBATypeCodePackage and platform:comprisesInterfacePart some OrgOmgSendingContext and platform:comprisesInterfacePart some OrgOmgCosNaming and platform:comprisesInterfacePart some OrgOmgCosNamingNamingContextExtPackage and platform:comprisesInterfacePart some OrgOmgCosNamingNamingContextPackage and platform:comprisesInterfacePart some OrgOmgPortableServer and platform:comprisesInterfacePart some OrgOmgPortableServerCurrentPackage and platform:comprisesInterfacePart some OrgOmgPortableServerPOAManagerPackage and platform:comprisesInterfacePart some OrgOmgPortableServerPOAPackage and platform:comprisesInterfacePart some OrgOmgPortableServerPortable and platform:comprisesInterfacePart some OrgOmgPortableServerServantLocatorPackage and platform:comprisesInterfacePart some OrgOmgDynamic and platform:comprisesInterfacePart some OrgOmgDynamicAny and platform:comprisesInterfacePart some OrgOmgDynamicAnyDynAnyFactoryPackage and platform:comprisesInterfacePart some OrgOmgDynamicAnyDynAnyPackage and platform:comprisesInterfacePart some OrgOmgIOP and platform:comprisesInterfacePart some OrgOmgIOPCodecFactoryPackage and platform:comprisesInterfacePart some OrgOmgIOPCodecPackage and platform:comprisesInterfacePart some OrgOmgMessaging and platform:comprisesInterfacePart some OrgOmgPortableInterceptor and platform:comprisesInterfacePart some OrgOmgPortableInterceptorORBInitInfoPackage and platform:comprisesInterfacePart some OrgOmgStubJavaRmi and platform:comprisesInterfacePart some OrgXmlSax and platform:comprisesInterfacePart some OrgXmlSaxHelpers and platform:comprisesInterfacePart some OrgXmlSaxExt and platform:comprisesInterfacePart some OrgIetfJgss</rdfs:comment>
	</owl:Class>
	<owl:Class rdf:about="&j2se-1_4;J2SE1_4ClassLibrary">
		<rdfs:subClassOf rdf:resource="&j2se-1_4;JavaLangClassLibrary"/>
		<rdfs:subClassOf rdf:resource="&j2se-1_4;JavaLangReflectClassLibrary"/>
		<rdfs:subClassOf rdf:resource="&j2se-1_4;JavaLangRefClassLibrary"/>
		<rdfs:subClassOf rdf:resource="&j2se-1_4;JavaIoClassLibrary"/>
		<rdfs:subClassOf rdf:resource="&j2se-1_4;JavaUtilClassLibrary"/>
		<rdfs:subClassOf rdf:resource="&j2se-1_4;JavaUtilLoggingClassLibrary"/>
		<rdfs:subClassOf rdf:resource="&j2se-1_4;JavaUtilJarClassLibrary"/>
		<rdfs:subClassOf rdf:resource="&j2se-1_4;JavaUtilZipClassLibrary"/>
		<rdfs:subClassOf rdf:resource="&j2se-1_4;JavaUtilPrefsClassLibrary"/>
		<rdfs:subClassOf rdf:resource="&j2se-1_4;JavaUtilRegexClassLibrary"/>
		<rdfs:subClassOf rdf:resource="&j2se-1_4;JavaNetClassLibrary"/>
		<rdfs:subClassOf rdf:resource="&j2se-1_4;JavaSecurityClassLibrary"/>
		<rdfs:subClassOf rdf:resource="&j2se-1_4;JavaSecurityCertClassLibrary"/>
		<rdfs:subClassOf rdf:resource="&j2se-1_4;JavaSecuritySpecClassLibrary"/>
		<rdfs:subClassOf rdf:resource="&j2se-1_4;JavaSecurityAclClassLibrary"/>
		<rdfs:subClassOf rdf:resource="&j2se-1_4;JavaSecurityInterfacesClassLibrary"/>
		<rdfs:subClassOf rdf:resource="&j2se-1_4;JavaNioClassLibrary"/>
		<rdfs:subClassOf rdf:resource="&j2se-1_4;JavaNioChannelsClassLibrary"/>
		<rdfs:subClassOf rdf:resource="&j2se-1_4;JavaNioChannelsSpiClassLibrary"/>
		<rdfs:subClassOf rdf:resource="&j2se-1_4;JavaNioCharsetClassLibrary"/>
		<rdfs:subClassOf rdf:resource="&j2se-1_4;JavaNioCharsetSpiClassLibrary"/>
		<rdfs:subClassOf rdf:resource="&j2se-1_4;JavaBeansClassLibrary"/>
		<rdfs:subClassOf rdf:resource="&j2se-1_4;JavaBeansBeancontextClassLibrary"/>
		<rdfs:subClassOf rdf:resource="&j2se-1_4;JavaAwtClassLibrary"/>
		<rdfs:subClassOf rdf:resource="&j2se-1_4;JavaAwtImageClassLibrary"/>
		<rdfs:subClassOf rdf:resource="&j2se-1_4;JavaAwtImageRenderableClassLibrary"/>
		<rdfs:subClassOf rdf:resource="&j2se-1_4;JavaAwtDatatransferClassLibrary"/>
		<rdfs:subClassOf rdf:resource="&j2se-1_4;JavaAwtDndClassLibrary"/>
		<rdfs:subClassOf rdf:resource="&j2se-1_4;JavaAwtEventClassLibrary"/>
		<rdfs:subClassOf rdf:resource="&j2se-1_4;JavaAwtImClassLibrary"/>
		<rdfs:subClassOf rdf:resource="&j2se-1_4;JavaAwtImSpiClassLibrary"/>
		<rdfs:subClassOf rdf:resource="&j2se-1_4;JavaAwtFontClassLibrary"/>
		<rdfs:subClassOf rdf:resource="&j2se-1_4;JavaAwtGeomClassLibrary"/>
		<rdfs:subClassOf rdf:resource="&j2se-1_4;JavaAwtColorClassLibrary"/>
		<rdfs:subClassOf rdf:resource="&j2se-1_4;JavaAwtPrintClassLibrary"/>
		<rdfs:subClassOf rdf:resource="&j2se-1_4;JavaTextClassLibrary"/>
		<rdfs:subClassOf rdf:resource="&j2se-1_4;JavaMathClassLibrary"/>
		<rdfs:subClassOf rdf:resource="&j2se-1_4;JavaAppletClassLibrary"/>
		<rdfs:subClassOf rdf:resource="&j2se-1_4;JavaRmiClassLibrary"/>
		<rdfs:subClassOf rdf:resource="&j2se-1_4;JavaRmiActivationClassLibrary"/>
		<rdfs:subClassOf rdf:resource="&j2se-1_4;JavaRmiServerClassLibrary"/>
		<rdfs:subClassOf rdf:resource="&j2se-1_4;JavaRmiDgcClassLibrary"/>
		<rdfs:subClassOf rdf:resource="&j2se-1_4;JavaRmiRegistryClassLibrary"/>
		<rdfs:subClassOf rdf:resource="&j2se-1_4;JavaSqlClassLibrary"/>
		<rdfs:subClassOf rdf:resource="&j2se-1_4;JavaxImageioClassLibrary"/>
		<rdfs:subClassOf rdf:resource="&j2se-1_4;JavaxImageioSpiClassLibrary"/>
		<rdfs:subClassOf rdf:resource="&j2se-1_4;JavaxImageioMetadataClassLibrary"/>
		<rdfs:subClassOf rdf:resource="&j2se-1_4;JavaxImageioStreamClassLibrary"/>
		<rdfs:subClassOf rdf:resource="&j2se-1_4;JavaxImageioEventClassLibrary"/>
		<rdfs:subClassOf rdf:resource="&j2se-1_4;JavaxImageioPluginsJpegClassLibrary"/>
		<rdfs:subClassOf rdf:resource="&j2se-1_4;JavaxAccessibilityClassLibrary"/>
		<rdfs:subClassOf rdf:resource="&j2se-1_4;JavaxSwingClassLibrary"/>
		<rdfs:subClassOf rdf:resource="&j2se-1_4;JavaxSwingPlafClassLibrary"/>
		<rdfs:subClassOf rdf:resource="&j2se-1_4;JavaxSwingPlafBasicClassLibrary"/>
		<rdfs:subClassOf rdf:resource="&j2se-1_4;JavaxSwingPlafMetalClassLibrary"/>
		<rdfs:subClassOf rdf:resource="&j2se-1_4;JavaxSwingPlafMultiClassLibrary"/>
		<rdfs:subClassOf rdf:resource="&j2se-1_4;JavaxSwingEventClassLibrary"/>
		<rdfs:subClassOf rdf:resource="&j2se-1_4;JavaxSwingBorderClassLibrary"/>
		<rdfs:subClassOf rdf:resource="&j2se-1_4;JavaxSwingTextClassLibrary"/>
		<rdfs:subClassOf rdf:resource="&j2se-1_4;JavaxSwingTextHtmlClassLibrary"/>
		<rdfs:subClassOf rdf:resource="&j2se-1_4;JavaxSwingTextHtmlParserClassLibrary"/>
		<rdfs:subClassOf rdf:resource="&j2se-1_4;JavaxSwingTextRtfClassLibrary"/>
		<rdfs:subClassOf rdf:resource="&j2se-1_4;JavaxSwingTableClassLibrary"/>
		<rdfs:subClassOf rdf:resource="&j2se-1_4;JavaxSwingUndoClassLibrary"/>
		<rdfs:subClassOf rdf:resource="&j2se-1_4;JavaxSwingTreeClassLibrary"/>
		<rdfs:subClassOf rdf:resource="&j2se-1_4;JavaxSwingFilechooserClassLibrary"/>
		<rdfs:subClassOf rdf:resource="&j2se-1_4;JavaxSwingColorchooserClassLibrary"/>
		<rdfs:subClassOf rdf:resource="&j2se-1_4;JavaxSoundSampledClassLibrary"/>
		<rdfs:subClassOf rdf:resource="&j2se-1_4;JavaxSoundSampledSpiClassLibrary"/>
		<rdfs:subClassOf rdf:resource="&j2se-1_4;JavaxSoundMidiClassLibrary"/>
		<rdfs:subClassOf rdf:resource="&j2se-1_4;JavaxSoundMidiSpiClassLibrary"/>
		<rdfs:subClassOf rdf:resource="&j2se-1_4;JavaxPrintClassLibrary"/>
		<rdfs:subClassOf rdf:resource="&j2se-1_4;JavaxPrintAttributeClassLibrary"/>
		<rdfs:subClassOf rdf:resource="&j2se-1_4;JavaxPrintAttributeStandardClassLibrary"/>
		<rdfs:subClassOf rdf:resource="&j2se-1_4;JavaxPrintEventClassLibrary"/>
		<rdfs:subClassOf rdf:resource="&j2se-1_4;JavaxSecurityAuthClassLibrary"/>
		<rdfs:subClassOf rdf:resource="&j2se-1_4;JavaxSecurityAuthX500ClassLibrary"/>
		<rdfs:subClassOf rdf:resource="&j2se-1_4;JavaxSecurityAuthCallbackClassLibrary"/>
		<rdfs:subClassOf rdf:resource="&j2se-1_4;JavaxSecurityAuthKerberosClassLibrary"/>
		<rdfs:subClassOf rdf:resource="&j2se-1_4;JavaxSecurityAuthLoginClassLibrary"/>
		<rdfs:subClassOf rdf:resource="&j2se-1_4;JavaxSecurityAuthSpiClassLibrary"/>
		<rdfs:subClassOf rdf:resource="&j2se-1_4;JavaxSecurityCertClassLibrary"/>
		<rdfs:subClassOf rdf:resource="&j2se-1_4;JavaxNamingClassLibrary"/>
		<rdfs:subClassOf rdf:resource="&j2se-1_4;JavaxNamingDirectoryClassLibrary"/>
		<rdfs:subClassOf rdf:resource="&j2se-1_4;JavaxNamingEventClassLibrary"/>
		<rdfs:subClassOf rdf:resource="&j2se-1_4;JavaxNamingLdapClassLibrary"/>
		<rdfs:subClassOf rdf:resource="&j2se-1_4;JavaxNamingSpiClassLibrary"/>
		<rdfs:subClassOf rdf:resource="&j2se-1_4;JavaxNetClassLibrary"/>
		<rdfs:subClassOf rdf:resource="&j2se-1_4;JavaxNetSslClassLibrary"/>
		<rdfs:subClassOf rdf:resource="&j2se-1_4;JavaxRmiClassLibrary"/>
		<rdfs:subClassOf rdf:resource="&j2se-1_4;JavaxRmiCORBAClassLibrary"/>
		<rdfs:subClassOf rdf:resource="&j2se-1_4;JavaxCryptoClassLibrary"/>
		<rdfs:subClassOf rdf:resource="&j2se-1_4;JavaxCryptoInterfacesClassLibrary"/>
		<rdfs:subClassOf rdf:resource="&j2se-1_4;JavaxCryptoSpecClassLibrary"/>
		<rdfs:subClassOf rdf:resource="&j2se-1_4;JavaxSqlClassLibrary"/>
		<rdfs:subClassOf rdf:resource="&j2se-1_4;JavaxTransactionClassLibrary"/>
		<rdfs:subClassOf rdf:resource="&j2se-1_4;JavaxTransactionXaClassLibrary"/>
		<rdfs:subClassOf rdf:resource="&j2se-1_4;JavaxXmlParsersClassLibrary"/>
		<rdfs:subClassOf rdf:resource="&j2se-1_4;JavaxXmlTransformClassLibrary"/>
		<rdfs:subClassOf rdf:resource="&j2se-1_4;JavaxXmlTransformDomClassLibrary"/>
		<rdfs:subClassOf rdf:resource="&j2se-1_4;JavaxXmlTransformSaxClassLibrary"/>
		<rdfs:subClassOf rdf:resource="&j2se-1_4;JavaxXmlTransformStreamClassLibrary"/>
		<rdfs:subClassOf rdf:resource="&j2se-1_4;OrgW3cDomClassLibrary"/>
		<rdfs:subClassOf rdf:resource="&j2se-1_4;OrgW3cDomCssClassLibrary"/>
		<rdfs:subClassOf rdf:resource="&j2se-1_4;OrgW3cDomStylesheetsClassLibrary"/>
		<rdfs:subClassOf rdf:resource="&j2se-1_4;OrgW3cDomViewsClassLibrary"/>
		<rdfs:subClassOf rdf:resource="&j2se-1_4;OrgW3cDomEventsClassLibrary"/>
		<rdfs:subClassOf rdf:resource="&j2se-1_4;OrgW3cDomHtmlClassLibrary"/>
		<rdfs:subClassOf rdf:resource="&j2se-1_4;OrgW3cDomTraversalClassLibrary"/>
		<rdfs:subClassOf rdf:resource="&j2se-1_4;OrgOmgCORBA_2_3ClassLibrary"/>
		<rdfs:subClassOf rdf:resource="&j2se-1_4;OrgOmgCORBA_2_3PortableClassLibrary"/>
		<rdfs:subClassOf rdf:resource="&j2se-1_4;OrgOmgCORBAClassLibrary"/>
		<rdfs:subClassOf rdf:resource="&j2se-1_4;OrgOmgCORBAPortableClassLibrary"/>
		<rdfs:subClassOf rdf:resource="&j2se-1_4;OrgOmgCORBADynAnyPackageClassLibrary"/>
		<rdfs:subClassOf rdf:resource="&j2se-1_4;OrgOmgCORBAORBPackageClassLibrary"/>
		<rdfs:subClassOf rdf:resource="&j2se-1_4;OrgOmgCORBATypeCodePackageClassLibrary"/>
		<rdfs:subClassOf rdf:resource="&j2se-1_4;OrgOmgSendingContextClassLibrary"/>
		<rdfs:subClassOf rdf:resource="&j2se-1_4;OrgOmgCosNamingClassLibrary"/>
		<rdfs:subClassOf rdf:resource="&j2se-1_4;OrgOmgCosNamingNamingContextExtPackageClassLibrary"/>
		<rdfs:subClassOf rdf:resource="&j2se-1_4;OrgOmgCosNamingNamingContextPackageClassLibrary"/>
		<rdfs:subClassOf rdf:resource="&j2se-1_4;OrgOmgPortableServerClassLibrary"/>
		<rdfs:subClassOf rdf:resource="&j2se-1_4;OrgOmgPortableServerCurrentPackageClassLibrary"/>
		<rdfs:subClassOf rdf:resource="&j2se-1_4;OrgOmgPortableServerPOAManagerPackageClassLibrary"/>
		<rdfs:subClassOf rdf:resource="&j2se-1_4;OrgOmgPortableServerPOAPackageClassLibrary"/>
		<rdfs:subClassOf rdf:resource="&j2se-1_4;OrgOmgPortableServerPortableClassLibrary"/>
		<rdfs:subClassOf rdf:resource="&j2se-1_4;OrgOmgPortableServerServantLocatorPackageClassLibrary"/>
		<rdfs:subClassOf rdf:resource="&j2se-1_4;OrgOmgDynamicClassLibrary"/>
		<rdfs:subClassOf rdf:resource="&j2se-1_4;OrgOmgDynamicAnyClassLibrary"/>
		<rdfs:subClassOf rdf:resource="&j2se-1_4;OrgOmgDynamicAnyDynAnyFactoryPackageClassLibrary"/>
		<rdfs:subClassOf rdf:resource="&j2se-1_4;OrgOmgDynamicAnyDynAnyPackageClassLibrary"/>
		<rdfs:subClassOf rdf:resource="&j2se-1_4;OrgOmgIOPClassLibrary"/>
		<rdfs:subClassOf rdf:resource="&j2se-1_4;OrgOmgIOPCodecFactoryPackageClassLibrary"/>
		<rdfs:subClassOf rdf:resource="&j2se-1_4;OrgOmgIOPCodecPackageClassLibrary"/>
		<rdfs:subClassOf rdf:resource="&j2se-1_4;OrgOmgMessagingClassLibrary"/>
		<rdfs:subClassOf rdf:resource="&j2se-1_4;OrgOmgPortableInterceptorClassLibrary"/>
		<rdfs:subClassOf rdf:resource="&j2se-1_4;OrgOmgPortableInterceptorORBInitInfoPackageClassLibrary"/>
		<rdfs:subClassOf rdf:resource="&j2se-1_4;OrgOmgStubJavaRmiClassLibrary"/>
		<rdfs:subClassOf rdf:resource="&j2se-1_4;OrgXmlSaxClassLibrary"/>
		<rdfs:subClassOf rdf:resource="&j2se-1_4;OrgXmlSaxHelpersClassLibrary"/>
		<rdfs:subClassOf rdf:resource="&j2se-1_4;OrgXmlSaxExtClassLibrary"/>
		<rdfs:subClassOf rdf:resource="&j2se-1_4;OrgIetfJgssClassLibrary"/>
		<rdfs:comment xml:lang="en">Java class library implementing the J2SE 1.4 API</rdfs:comment>
		<rdfs:comment xml:lang="OWLManchester">platform:implementsInterface some J2SE1_4API</rdfs:comment>
	</owl:Class>
	<owl:Class rdf:about="&j2se-1_4;J2SE1_4BytecodeFormat">
		<owl:equivalentClass rdf:resource="&j2me-pp-1_1;J2MEPP1_1BytecodeFormat"/>
		<rdfs:subClassOf rdf:resource="&j2se-1_3;J2SE1_3BytecodeFormat"/>
		<rdfs:comment xml:lang="en">J2SE 1.4 bytecode format</rdfs:comment>
		<rdfs:comment xml:lang="OWLManchester">java:majorVersionNumber some xsd:integer[>="48"^^xsd:integer] and java:preverified value false</rdfs:comment>
	</owl:Class>
	<j2se-1_4:J2SE1_4BytecodeFormat rdf:about="&j2se-1_4;theJ2SE1_4BytecodeFormat">
		<java:preverified rdf:datatype="http://www.w3.org/2001/XMLSchema#boolean">false</java:preverified>
		<java:minorVersionNumber rdf:datatype="http://www.w3.org/2001/XMLSchema#integer">3</java:minorVersionNumber>
		<java:majorVersionNumber rdf:datatype="http://www.w3.org/2001/XMLSchema#integer">48</java:majorVersionNumber>
	</j2se-1_4:J2SE1_4BytecodeFormat>
	<j2se-1_4:J2SE1_4API rdf:about="&j2se-1_4;theJ2SE1_4API">
		<platform:comprisesInterfacePart rdf:resource="&j2se-1_4;theOrgIetfJgssPart"/>
		<platform:comprisesInterfacePart rdf:resource="&j2se-1_4;theOrgXmlSaxExtPart"/>
		<platform:comprisesInterfacePart rdf:resource="&j2se-1_4;theOrgXmlSaxHelpersPart"/>
		<platform:comprisesInterfacePart rdf:resource="&j2se-1_4;theOrgXmlSaxPart"/>
		<platform:comprisesInterfacePart rdf:resource="&j2se-1_4;theOrgOmgStubJavaRmiPart"/>
		<platform:comprisesInterfacePart rdf:resource="&j2se-1_4;theOrgOmgPortableInterceptorORBInitInfoPackagePart"/>
		<platform:comprisesInterfacePart rdf:resource="&j2se-1_4;theOrgOmgPortableInterceptorPart"/>
		<platform:comprisesInterfacePart rdf:resource="&j2se-1_4;theOrgOmgMessagingPart"/>
		<platform:comprisesInterfacePart rdf:resource="&j2se-1_4;theOrgOmgIOPCodecPackagePart"/>
		<platform:comprisesInterfacePart rdf:resource="&j2se-1_4;theOrgOmgIOPCodecFactoryPackagePart"/>
		<platform:comprisesInterfacePart rdf:resource="&j2se-1_4;theOrgOmgIOPPart"/>
		<platform:comprisesInterfacePart rdf:resource="&j2se-1_4;theOrgOmgDynamicAnyDynAnyPackagePart"/>
		<platform:comprisesInterfacePart rdf:resource="&j2se-1_4;theOrgOmgDynamicAnyDynAnyFactoryPackagePart"/>
		<platform:comprisesInterfacePart rdf:resource="&j2se-1_4;theOrgOmgDynamicAnyPart"/>
		<platform:comprisesInterfacePart rdf:resource="&j2se-1_4;theOrgOmgDynamicPart"/>
		<platform:comprisesInterfacePart rdf:resource="&j2se-1_4;theOrgOmgPortableServerServantLocatorPackagePart"/>
		<platform:comprisesInterfacePart rdf:resource="&j2se-1_4;theOrgOmgPortableServerPortablePart"/>
		<platform:comprisesInterfacePart rdf:resource="&j2se-1_4;theOrgOmgPortableServerPOAPackagePart"/>
		<platform:comprisesInterfacePart rdf:resource="&j2se-1_4;theOrgOmgPortableServerPOAManagerPackagePart"/>
		<platform:comprisesInterfacePart rdf:resource="&j2se-1_4;theOrgOmgPortableServerCurrentPackagePart"/>
		<platform:comprisesInterfacePart rdf:resource="&j2se-1_4;theOrgOmgPortableServerPart"/>
		<platform:comprisesInterfacePart rdf:resource="&j2se-1_4;theOrgOmgCosNamingNamingContextPackagePart"/>
		<platform:comprisesInterfacePart rdf:resource="&j2se-1_4;theOrgOmgCosNamingNamingContextExtPackagePart"/>
		<platform:comprisesInterfacePart rdf:resource="&j2se-1_4;theOrgOmgCosNamingPart"/>
		<platform:comprisesInterfacePart rdf:resource="&j2se-1_4;theOrgOmgSendingContextPart"/>
		<platform:comprisesInterfacePart rdf:resource="&j2se-1_4;theOrgOmgCORBATypeCodePackagePart"/>
		<platform:comprisesInterfacePart rdf:resource="&j2se-1_4;theOrgOmgCORBAORBPackagePart"/>
		<platform:comprisesInterfacePart rdf:resource="&j2se-1_4;theOrgOmgCORBADynAnyPackagePart"/>
		<platform:comprisesInterfacePart rdf:resource="&j2se-1_4;theOrgOmgCORBAPortablePart"/>
		<platform:comprisesInterfacePart rdf:resource="&j2se-1_4;theOrgOmgCORBAPart"/>
		<platform:comprisesInterfacePart rdf:resource="&j2se-1_4;theOrgOmgCORBA_2_3PortablePart"/>
		<platform:comprisesInterfacePart rdf:resource="&j2se-1_4;theOrgOmgCORBA_2_3Part"/>
		<platform:comprisesInterfacePart rdf:resource="&j2se-1_4;theOrgW3cDomTraversalPart"/>
		<platform:comprisesInterfacePart rdf:resource="&j2se-1_4;theOrgW3cDomHtmlPart"/>
		<platform:comprisesInterfacePart rdf:resource="&j2se-1_4;theOrgW3cDomEventsPart"/>
		<platform:comprisesInterfacePart rdf:resource="&j2se-1_4;theOrgW3cDomViewsPart"/>
		<platform:comprisesInterfacePart rdf:resource="&j2se-1_4;theOrgW3cDomStylesheetsPart"/>
		<platform:comprisesInterfacePart rdf:resource="&j2se-1_4;theOrgW3cDomCssPart"/>
		<platform:comprisesInterfacePart rdf:resource="&j2se-1_4;theOrgW3cDomPart"/>
		<platform:comprisesInterfacePart rdf:resource="&j2se-1_4;theJavaxXmlTransformStreamPart"/>
		<platform:comprisesInterfacePart rdf:resource="&j2se-1_4;theJavaxXmlTransformSaxPart"/>
		<platform:comprisesInterfacePart rdf:resource="&j2se-1_4;theJavaxXmlTransformDomPart"/>
		<platform:comprisesInterfacePart rdf:resource="&j2se-1_4;theJavaxXmlTransformPart"/>
		<platform:comprisesInterfacePart rdf:resource="&j2se-1_4;theJavaxXmlParsersPart"/>
		<platform:comprisesInterfacePart rdf:resource="&j2se-1_4;theJavaxTransactionXaPart"/>
		<platform:comprisesInterfacePart rdf:resource="&j2se-1_4;theJavaxTransactionPart"/>
		<platform:comprisesInterfacePart rdf:resource="&j2se-1_4;theJavaxSqlPart"/>
		<platform:comprisesInterfacePart rdf:resource="&j2se-1_4;theJavaxCryptoSpecPart"/>
		<platform:comprisesInterfacePart rdf:resource="&j2se-1_4;theJavaxCryptoInterfacesPart"/>
		<platform:comprisesInterfacePart rdf:resource="&j2se-1_4;theJavaxCryptoPart"/>
		<platform:comprisesInterfacePart rdf:resource="&j2se-1_4;theJavaxRmiCORBAPart"/>
		<platform:comprisesInterfacePart rdf:resource="&j2se-1_4;theJavaxRmiPart"/>
		<platform:comprisesInterfacePart rdf:resource="&j2se-1_4;theJavaxNetSslPart"/>
		<platform:comprisesInterfacePart rdf:resource="&j2se-1_4;theJavaxNetPart"/>
		<platform:comprisesInterfacePart rdf:resource="&j2se-1_4;theJavaxNamingSpiPart"/>
		<platform:comprisesInterfacePart rdf:resource="&j2se-1_4;theJavaxNamingLdapPart"/>
		<platform:comprisesInterfacePart rdf:resource="&j2se-1_4;theJavaxNamingEventPart"/>
		<platform:comprisesInterfacePart rdf:resource="&j2se-1_4;theJavaxNamingDirectoryPart"/>
		<platform:comprisesInterfacePart rdf:resource="&j2se-1_4;theJavaxNamingPart"/>
		<platform:comprisesInterfacePart rdf:resource="&j2se-1_4;theJavaxSecurityCertPart"/>
		<platform:comprisesInterfacePart rdf:resource="&j2se-1_4;theJavaxSecurityAuthSpiPart"/>
		<platform:comprisesInterfacePart rdf:resource="&j2se-1_4;theJavaxSecurityAuthLoginPart"/>
		<platform:comprisesInterfacePart rdf:resource="&j2se-1_4;theJavaxSecurityAuthKerberosPart"/>
		<platform:comprisesInterfacePart rdf:resource="&j2se-1_4;theJavaxSecurityAuthCallbackPart"/>
		<platform:comprisesInterfacePart rdf:resource="&j2se-1_4;theJavaxSecurityAuthX500Part"/>
		<platform:comprisesInterfacePart rdf:resource="&j2se-1_4;theJavaxSecurityAuthPart"/>
		<platform:comprisesInterfacePart rdf:resource="&j2se-1_4;theJavaxPrintEventPart"/>
		<platform:comprisesInterfacePart rdf:resource="&j2se-1_4;theJavaxPrintAttributeStandardPart"/>
		<platform:comprisesInterfacePart rdf:resource="&j2se-1_4;theJavaxPrintAttributePart"/>
		<platform:comprisesInterfacePart rdf:resource="&j2se-1_4;theJavaxPrintPart"/>
		<platform:comprisesInterfacePart rdf:resource="&j2se-1_4;theJavaxSoundMidiSpiPart"/>
		<platform:comprisesInterfacePart rdf:resource="&j2se-1_4;theJavaxSoundMidiPart"/>
		<platform:comprisesInterfacePart rdf:resource="&j2se-1_4;theJavaxSoundSampledSpiPart"/>
		<platform:comprisesInterfacePart rdf:resource="&j2se-1_4;theJavaxSoundSampledPart"/>
		<platform:comprisesInterfacePart rdf:resource="&j2se-1_4;theJavaxSwingColorchooserPart"/>
		<platform:comprisesInterfacePart rdf:resource="&j2se-1_4;theJavaxSwingFilechooserPart"/>
		<platform:comprisesInterfacePart rdf:resource="&j2se-1_4;theJavaxSwingTreePart"/>
		<platform:comprisesInterfacePart rdf:resource="&j2se-1_4;theJavaxSwingUndoPart"/>
		<platform:comprisesInterfacePart rdf:resource="&j2se-1_4;theJavaxSwingTablePart"/>
		<platform:comprisesInterfacePart rdf:resource="&j2se-1_4;theJavaxSwingTextRtfPart"/>
		<platform:comprisesInterfacePart rdf:resource="&j2se-1_4;theJavaxSwingTextHtmlParserPart"/>
		<platform:comprisesInterfacePart rdf:resource="&j2se-1_4;theJavaxSwingTextHtmlPart"/>
		<platform:comprisesInterfacePart rdf:resource="&j2se-1_4;theJavaxSwingTextPart"/>
		<platform:comprisesInterfacePart rdf:resource="&j2se-1_4;theJavaxSwingBorderPart"/>
		<platform:comprisesInterfacePart rdf:resource="&j2se-1_4;theJavaxSwingEventPart"/>
		<platform:comprisesInterfacePart rdf:resource="&j2se-1_4;theJavaxSwingPlafMultiPart"/>
		<platform:comprisesInterfacePart rdf:resource="&j2se-1_4;theJavaxSwingPlafMetalPart"/>
		<platform:comprisesInterfacePart rdf:resource="&j2se-1_4;theJavaxSwingPlafBasicPart"/>
		<platform:comprisesInterfacePart rdf:resource="&j2se-1_4;theJavaxSwingPlafPart"/>
		<platform:comprisesInterfacePart rdf:resource="&j2se-1_4;theJavaxSwingPart"/>
		<platform:comprisesInterfacePart rdf:resource="&j2se-1_4;theJavaxAccessibilityPart"/>
		<platform:comprisesInterfacePart rdf:resource="&j2se-1_4;theJavaxImageioPluginsJpegPart"/>
		<platform:comprisesInterfacePart rdf:resource="&j2se-1_4;theJavaxImageioEventPart"/>
		<platform:comprisesInterfacePart rdf:resource="&j2se-1_4;theJavaxImageioStreamPart"/>
		<platform:comprisesInterfacePart rdf:resource="&j2se-1_4;theJavaxImageioMetadataPart"/>
		<platform:comprisesInterfacePart rdf:resource="&j2se-1_4;theJavaxImageioSpiPart"/>
		<platform:comprisesInterfacePart rdf:resource="&j2se-1_4;theJavaxImageioPart"/>
		<platform:comprisesInterfacePart rdf:resource="&j2se-1_4;theJavaSqlPart"/>
		<platform:comprisesInterfacePart rdf:resource="&j2se-1_4;theJavaRmiRegistryPart"/>
		<platform:comprisesInterfacePart rdf:resource="&j2se-1_4;theJavaRmiDgcPart"/>
		<platform:comprisesInterfacePart rdf:resource="&j2se-1_4;theJavaRmiServerPart"/>
		<platform:comprisesInterfacePart rdf:resource="&j2se-1_4;theJavaRmiActivationPart"/>
		<platform:comprisesInterfacePart rdf:resource="&j2se-1_4;theJavaRmiPart"/>
		<platform:comprisesInterfacePart rdf:resource="&j2se-1_4;theJavaAppletPart"/>
		<platform:comprisesInterfacePart rdf:resource="&j2se-1_4;theJavaMathPart"/>
		<platform:comprisesInterfacePart rdf:resource="&j2se-1_4;theJavaTextPart"/>
		<platform:comprisesInterfacePart rdf:resource="&j2se-1_4;theJavaAwtPrintPart"/>
		<platform:comprisesInterfacePart rdf:resource="&j2se-1_4;theJavaAwtColorPart"/>
		<platform:comprisesInterfacePart rdf:resource="&j2se-1_4;theJavaAwtGeomPart"/>
		<platform:comprisesInterfacePart rdf:resource="&j2se-1_4;theJavaAwtFontPart"/>
		<platform:comprisesInterfacePart rdf:resource="&j2se-1_4;theJavaAwtImSpiPart"/>
		<platform:comprisesInterfacePart rdf:resource="&j2se-1_4;theJavaAwtImPart"/>
		<platform:comprisesInterfacePart rdf:resource="&j2se-1_4;theJavaAwtEventPart"/>
		<platform:comprisesInterfacePart rdf:resource="&j2se-1_4;theJavaAwtDndPart"/>
		<platform:comprisesInterfacePart rdf:resource="&j2se-1_4;theJavaAwtDatatransferPart"/>
		<platform:comprisesInterfacePart rdf:resource="&j2se-1_4;theJavaAwtImageRenderablePart"/>
		<platform:comprisesInterfacePart rdf:resource="&j2se-1_4;theJavaAwtImagePart"/>
		<platform:comprisesInterfacePart rdf:resource="&j2se-1_4;theJavaAwtPart"/>
		<platform:comprisesInterfacePart rdf:resource="&j2se-1_4;theJavaBeansBeancontextPart"/>
		<platform:comprisesInterfacePart rdf:resource="&j2se-1_4;theJavaBeansPart"/>
		<platform:comprisesInterfacePart rdf:resource="&j2se-1_4;theJavaNioCharsetSpiPart"/>
		<platform:comprisesInterfacePart rdf:resource="&j2se-1_4;theJavaNioCharsetPart"/>
		<platform:comprisesInterfacePart rdf:resource="&j2se-1_4;theJavaNioChannelsSpiPart"/>
		<platform:comprisesInterfacePart rdf:resource="&j2se-1_4;theJavaNioChannelsPart"/>
		<platform:comprisesInterfacePart rdf:resource="&j2se-1_4;theJavaNioPart"/>
		<platform:comprisesInterfacePart rdf:resource="&j2se-1_4;theJavaSecurityInterfacesPart"/>
		<platform:comprisesInterfacePart rdf:resource="&j2se-1_4;theJavaSecurityAclPart"/>
		<platform:comprisesInterfacePart rdf:resource="&j2se-1_4;theJavaSecuritySpecPart"/>
		<platform:comprisesInterfacePart rdf:resource="&j2se-1_4;theJavaSecurityCertPart"/>
		<platform:comprisesInterfacePart rdf:resource="&j2se-1_4;theJavaSecurityPart"/>
		<platform:comprisesInterfacePart rdf:resource="&j2se-1_4;theJavaNetPart"/>
		<platform:comprisesInterfacePart rdf:resource="&j2se-1_4;theJavaUtilRegexPart"/>
		<platform:comprisesInterfacePart rdf:resource="&j2se-1_4;theJavaUtilPrefsPart"/>
		<platform:comprisesInterfacePart rdf:resource="&j2se-1_4;theJavaUtilZipPart"/>
		<platform:comprisesInterfacePart rdf:resource="&j2se-1_4;theJavaUtilJarPart"/>
		<platform:comprisesInterfacePart rdf:resource="&j2se-1_4;theJavaUtilLoggingPart"/>
		<platform:comprisesInterfacePart rdf:resource="&j2se-1_4;theJavaUtilPart"/>
		<platform:comprisesInterfacePart rdf:resource="&j2se-1_4;theJavaIoPart"/>
		<platform:comprisesInterfacePart rdf:resource="&j2se-1_4;theJavaLangRefPart"/>
		<platform:comprisesInterfacePart rdf:resource="&j2se-1_4;theJavaLangReflectPart"/>
		<platform:comprisesInterfacePart rdf:resource="&j2se-1_4;theJavaLangPart"/>
	</j2se-1_4:J2SE1_4API>
	<owl:Class rdf:about="&j2se-1_4;J2SE1_4VM">
		<owl:equivalentClass>
			<owl:Restriction>
				<owl:onProperty rdf:resource="&platform;implementsInterface"/>
				<owl:someValuesFrom rdf:resource="&j2se-1_4;J2SE1_4BytecodeFormat"/>
			</owl:Restriction>
		</owl:equivalentClass>
		<rdfs:subClassOf rdf:resource="&java;JavaVM"/>
		<rdfs:comment xml:lang="en">J2SE 1.4 virtual machine</rdfs:comment>
	</owl:Class>
	<owl:Class rdf:about="&j2se-1_4;J2SE1_4JRE">
		<owl:equivalentClass>
			<owl:Class >
				<owl:intersectionOf rdf:parseType="Collection">
					<owl:Restriction>
						<owl:onProperty rdf:resource="&platform;providesFeature"/>
						<owl:someValuesFrom rdf:resource="&j2se-1_4;J2SE1_4ClassLibrary"/>
					</owl:Restriction>
					<owl:Restriction>
						<owl:onProperty rdf:resource="&platform;providesFeature"/>
						<owl:someValuesFrom rdf:resource="&j2se-1_4;J2SE1_4VM"/>
					</owl:Restriction>
				</owl:intersectionOf>
			</owl:Class>
		</owl:equivalentClass>
		<rdfs:subClassOf rdf:resource="&java;JRE"/>
		<rdfs:comment xml:lang="en">J2SE 1.4 Java Runtime Environment</rdfs:comment>
	</owl:Class>
	<owl:Class rdf:about="&j2se-1_4;JavaLang">
		<rdfs:subClassOf rdf:resource="&j2me-pp-1_1;JavaLang"/>
		<rdfs:subClassOf rdf:resource="&j2se-1_3;JavaLang"/>
		<rdfs:seeAlso rdf:resource="&j2se-1_4;JavaNet"/>
		<rdfs:seeAlso rdf:resource="&j2se-1_4;JavaSecurity"/>
		<rdfs:seeAlso rdf:resource="&j2se-1_4;JavaUtil"/>
		<rdfs:seeAlso rdf:resource="&j2se-1_4;JavaIo"/>
		<rdfs:seeAlso rdf:resource="&j2se-1_4;JavaLangReflect"/>
		<rdfs:comment xml:lang="en">Java API part implementing the java.lang package for J2SE 1.4</rdfs:comment>
	</owl:Class>
	<owl:Class rdf:about="&j2se-1_4;JavaLangReflect">
		<owl:equivalentClass rdf:resource="&j2me-pp-1_1;JavaLangReflect"/>
		<rdfs:subClassOf rdf:resource="&j2se-1_3;JavaLangReflect"/>
		<rdfs:seeAlso rdf:resource="&j2se-1_4;JavaSecurity"/>
		<rdfs:seeAlso rdf:resource="&j2se-1_4;JavaLang"/>
		<rdfs:seeAlso rdf:resource="&j2se-1_4;JavaIo"/>
		<rdfs:comment xml:lang="en">Java API part implementing the java.lang.reflect package for J2SE 1.4</rdfs:comment>
	</owl:Class>
	<owl:Class rdf:about="&j2se-1_4;JavaLangRef">
		<owl:equivalentClass rdf:resource="&j2me-pp-1_1;JavaLangRef"/>
		<owl:equivalentClass rdf:resource="&j2se-1_3;JavaLangRef"/>
		<rdfs:subClassOf rdf:resource="&java;JavaAPIPart"/>
		<rdfs:seeAlso rdf:resource="&j2se-1_4;JavaLang"/>
		<rdfs:comment xml:lang="en">Java API part implementing the java.lang.ref package for J2SE 1.4</rdfs:comment>
	</owl:Class>
	<owl:Class rdf:about="&j2se-1_4;JavaIo">
		<rdfs:subClassOf rdf:resource="&j2me-pp-1_1;JavaIo"/>
		<rdfs:subClassOf rdf:resource="&j2se-1_3;JavaIo"/>
		<rdfs:seeAlso rdf:resource="&j2se-1_4;JavaNet"/>
		<rdfs:seeAlso rdf:resource="&j2se-1_4;JavaNioChannels"/>
		<rdfs:seeAlso rdf:resource="&j2se-1_4;JavaNioCharset"/>
		<rdfs:seeAlso rdf:resource="&j2se-1_4;JavaSecurity"/>
		<rdfs:seeAlso rdf:resource="&j2se-1_4;JavaUtil"/>
		<rdfs:seeAlso rdf:resource="&j2se-1_4;JavaLang"/>
		<rdfs:comment xml:lang="en">Java API part implementing the java.io package for J2SE 1.4</rdfs:comment>
	</owl:Class>
	<owl:Class rdf:about="&j2se-1_4;JavaUtil">
		<rdfs:subClassOf rdf:resource="&j2me-pp-1_1;JavaUtil"/>
		<rdfs:subClassOf rdf:resource="&j2se-1_3;JavaUtil"/>
		<rdfs:seeAlso rdf:resource="&j2se-1_4;JavaSecurity"/>
		<rdfs:seeAlso rdf:resource="&j2se-1_4;JavaLang"/>
		<rdfs:seeAlso rdf:resource="&j2se-1_4;JavaIo"/>
		<rdfs:comment xml:lang="en">Java API part implementing the java.util package for J2SE 1.4</rdfs:comment>
	</owl:Class>
	<owl:Class rdf:about="&j2se-1_4;JavaUtilLogging">
		<rdfs:subClassOf rdf:resource="&java;JavaAPIPart"/>
		<rdfs:seeAlso rdf:resource="&j2se-1_4;JavaUtil"/>
		<rdfs:seeAlso rdf:resource="&j2se-1_4;JavaSecurity"/>
		<rdfs:seeAlso rdf:resource="&j2se-1_4;JavaLang"/>
		<rdfs:seeAlso rdf:resource="&j2se-1_4;JavaBeans"/>
		<rdfs:seeAlso rdf:resource="&j2se-1_4;JavaIo"/>
		<rdfs:comment xml:lang="en">Java API part implementing the java.util.logging package for J2SE 1.4</rdfs:comment>
	</owl:Class>
	<owl:Class rdf:about="&j2se-1_4;JavaUtilJar">
		<owl:equivalentClass rdf:resource="&j2me-pp-1_1;JavaUtilJar"/>
		<rdfs:subClassOf rdf:resource="&j2se-1_3;JavaUtilJar"/>
		<rdfs:seeAlso rdf:resource="&j2se-1_4;JavaUtil"/>
		<rdfs:seeAlso rdf:resource="&j2se-1_4;JavaLang"/>
		<rdfs:seeAlso rdf:resource="&j2se-1_4;JavaIo"/>
		<rdfs:seeAlso rdf:resource="&j2se-1_4;JavaUtilZip"/>
		<rdfs:comment xml:lang="en">Java API part implementing the java.util.jar package for J2SE 1.4</rdfs:comment>
	</owl:Class>
	<owl:Class rdf:about="&j2se-1_4;JavaUtilZip">
		<owl:equivalentClass rdf:resource="&j2me-pp-1_1;JavaUtilZip"/>
		<rdfs:subClassOf rdf:resource="&j2se-1_3;JavaUtilZip"/>
		<rdfs:seeAlso rdf:resource="&j2se-1_4;JavaUtil"/>
		<rdfs:seeAlso rdf:resource="&j2se-1_4;JavaLang"/>
		<rdfs:seeAlso rdf:resource="&j2se-1_4;JavaIo"/>
		<rdfs:comment xml:lang="en">Java API part implementing the java.util.zip package for J2SE 1.4</rdfs:comment>
	</owl:Class>
	<owl:Class rdf:about="&j2se-1_4;JavaUtilPrefs">
		<rdfs:subClassOf rdf:resource="&java;JavaAPIPart"/>
		<rdfs:seeAlso rdf:resource="&j2se-1_4;JavaUtil"/>
		<rdfs:seeAlso rdf:resource="&j2se-1_4;JavaLang"/>
		<rdfs:seeAlso rdf:resource="&j2se-1_4;JavaIo"/>
		<rdfs:comment xml:lang="en">Java API part implementing the java.util.prefs package for J2SE 1.4</rdfs:comment>
	</owl:Class>
	<owl:Class rdf:about="&j2se-1_4;JavaUtilRegex">
		<rdfs:subClassOf rdf:resource="&java;JavaAPIPart"/>
		<rdfs:seeAlso rdf:resource="&j2se-1_4;JavaLang"/>
		<rdfs:seeAlso rdf:resource="&j2se-1_4;JavaIo"/>
		<rdfs:comment xml:lang="en">Java API part implementing the java.util.regex package for J2SE 1.4</rdfs:comment>
	</owl:Class>
	<owl:Class rdf:about="&j2se-1_4;JavaNet">
		<rdfs:subClassOf rdf:resource="&j2me-pp-1_1;JavaNet"/>
		<rdfs:subClassOf rdf:resource="&j2se-1_3;JavaNet"/>
		<rdfs:seeAlso rdf:resource="&j2se-1_4;JavaUtil"/>
		<rdfs:seeAlso rdf:resource="&j2se-1_4;JavaSecurity"/>
		<rdfs:seeAlso rdf:resource="&j2se-1_4;JavaLang"/>
		<rdfs:seeAlso rdf:resource="&j2se-1_4;JavaIo"/>
		<rdfs:seeAlso rdf:resource="&j2se-1_4;JavaNioChannels"/>
		<rdfs:seeAlso rdf:resource="&j2se-1_4;JavaUtilJar"/>
		<rdfs:comment xml:lang="en">Java API part implementing the java.net package for J2SE 1.4</rdfs:comment>
	</owl:Class>
	<owl:Class rdf:about="&j2se-1_4;JavaSecurity">
		<rdfs:subClassOf rdf:resource="&j2me-pp-1_1;JavaSecurity"/>
		<rdfs:subClassOf rdf:resource="&j2se-1_3;JavaSecurity"/>
		<rdfs:seeAlso rdf:resource="&j2se-1_4;JavaSecurityCert"/>
		<rdfs:seeAlso rdf:resource="&j2se-1_4;JavaSecuritySpec"/>
		<rdfs:seeAlso rdf:resource="&j2se-1_4;JavaUtil"/>
		<rdfs:seeAlso rdf:resource="&j2se-1_4;JavaLang"/>
		<rdfs:seeAlso rdf:resource="&j2se-1_4;JavaIo"/>
		<rdfs:seeAlso rdf:resource="&j2se-1_4;JavaNet"/>
		<rdfs:comment xml:lang="en">Java API part implementing the java.security package for J2SE 1.4</rdfs:comment>
	</owl:Class>
	<owl:Class rdf:about="&j2se-1_4;JavaSecurityCert">
		<rdfs:subClassOf rdf:resource="&j2me-pp-1_1;JavaSecurityCert"/>
		<rdfs:subClassOf rdf:resource="&j2se-1_3;JavaSecurityCert"/>
		<rdfs:seeAlso rdf:resource="&j2se-1_4;JavaMath"/>
		<rdfs:seeAlso rdf:resource="&j2se-1_4;JavaUtil"/>
		<rdfs:seeAlso rdf:resource="&j2se-1_4;JavaSecurity"/>
		<rdfs:seeAlso rdf:resource="&j2se-1_4;JavaLang"/>
		<rdfs:seeAlso rdf:resource="&j2se-1_4;JavaxSecurityAuthX500"/>
		<rdfs:seeAlso rdf:resource="&j2se-1_4;JavaIo"/>
		<rdfs:comment xml:lang="en">Java API part implementing the java.security.cert package for J2SE 1.4</rdfs:comment>
	</owl:Class>
	<owl:Class rdf:about="&j2se-1_4;JavaSecuritySpec">
		<rdfs:subClassOf rdf:resource="&j2me-pp-1_1;JavaSecuritySpec"/>
		<rdfs:subClassOf rdf:resource="&j2se-1_3;JavaSecuritySpec"/>
		<rdfs:seeAlso rdf:resource="&j2se-1_4;JavaSecurity"/>
		<rdfs:seeAlso rdf:resource="&j2se-1_4;JavaLang"/>
		<rdfs:seeAlso rdf:resource="&j2se-1_4;JavaSecurityInterfaces"/>
		<rdfs:seeAlso rdf:resource="&j2se-1_4;JavaMath"/>
		<rdfs:comment xml:lang="en">Java API part implementing the java.security.spec package for J2SE 1.4</rdfs:comment>
	</owl:Class>
	<owl:Class rdf:about="&j2se-1_4;JavaSecurityAcl">
		<owl:equivalentClass rdf:resource="&j2me-pp-1_1;JavaSecurityAcl"/>
		<rdfs:subClassOf rdf:resource="&j2se-1_3;JavaSecurityAcl"/>
		<rdfs:seeAlso rdf:resource="&j2se-1_4;JavaSecurity"/>
		<rdfs:seeAlso rdf:resource="&j2se-1_4;JavaUtil"/>
		<rdfs:seeAlso rdf:resource="&j2se-1_4;JavaLang"/>
		<rdfs:comment xml:lang="en">Java API part implementing the java.security.acl package for J2SE 1.4</rdfs:comment>
	</owl:Class>
	<owl:Class rdf:about="&j2se-1_4;JavaSecurityInterfaces">
		<rdfs:subClassOf rdf:resource="&j2me-pp-1_1;JavaSecurityInterfaces"/>
		<rdfs:subClassOf rdf:resource="&j2se-1_3;JavaSecurityInterfaces"/>
		<rdfs:seeAlso rdf:resource="&j2se-1_4;JavaSecurity"/>
		<rdfs:seeAlso rdf:resource="&j2se-1_4;JavaMath"/>
		<rdfs:comment xml:lang="en">Java API part implementing the java.security.interfaces package for J2SE 1.4</rdfs:comment>
	</owl:Class>
	<owl:Class rdf:about="&j2se-1_4;JavaNio">
		<rdfs:subClassOf rdf:resource="&java;JavaAPIPart"/>
		<rdfs:seeAlso rdf:resource="&j2se-1_4;JavaLang"/>
		<rdfs:comment xml:lang="en">Java API part implementing the java.nio package for J2SE 1.4</rdfs:comment>
	</owl:Class>
	<owl:Class rdf:about="&j2se-1_4;JavaNioChannels">
		<rdfs:subClassOf rdf:resource="&java;JavaAPIPart"/>
		<rdfs:seeAlso rdf:resource="&j2se-1_4;JavaNet"/>
		<rdfs:seeAlso rdf:resource="&j2se-1_4;JavaNioCharset"/>
		<rdfs:seeAlso rdf:resource="&j2se-1_4;JavaUtil"/>
		<rdfs:seeAlso rdf:resource="&j2se-1_4;JavaLang"/>
		<rdfs:seeAlso rdf:resource="&j2se-1_4;JavaIo"/>
		<rdfs:seeAlso rdf:resource="&j2se-1_4;JavaNio"/>
		<rdfs:seeAlso rdf:resource="&j2se-1_4;JavaNioChannelsSpi"/>
		<rdfs:comment xml:lang="en">Java API part implementing the java.nio.channels package for J2SE 1.4</rdfs:comment>
	</owl:Class>
	<owl:Class rdf:about="&j2se-1_4;JavaNioChannelsSpi">
		<rdfs:subClassOf rdf:resource="&java;JavaAPIPart"/>
		<rdfs:seeAlso rdf:resource="&j2se-1_4;JavaUtil"/>
		<rdfs:seeAlso rdf:resource="&j2se-1_4;JavaLang"/>
		<rdfs:seeAlso rdf:resource="&j2se-1_4;JavaNioChannels"/>
		<rdfs:comment xml:lang="en">Java API part implementing the java.nio.channels.spi package for J2SE 1.4</rdfs:comment>
	</owl:Class>
	<owl:Class rdf:about="&j2se-1_4;JavaNioCharset">
		<rdfs:subClassOf rdf:resource="&java;JavaAPIPart"/>
		<rdfs:seeAlso rdf:resource="&j2se-1_4;JavaUtil"/>
		<rdfs:seeAlso rdf:resource="&j2se-1_4;JavaLang"/>
		<rdfs:seeAlso rdf:resource="&j2se-1_4;JavaIo"/>
		<rdfs:seeAlso rdf:resource="&j2se-1_4;JavaNio"/>
		<rdfs:comment xml:lang="en">Java API part implementing the java.nio.charset package for J2SE 1.4</rdfs:comment>
	</owl:Class>
	<owl:Class rdf:about="&j2se-1_4;JavaNioCharsetSpi">
		<rdfs:subClassOf rdf:resource="&java;JavaAPIPart"/>
		<rdfs:seeAlso rdf:resource="&j2se-1_4;JavaNioCharset"/>
		<rdfs:seeAlso rdf:resource="&j2se-1_4;JavaUtil"/>
		<rdfs:seeAlso rdf:resource="&j2se-1_4;JavaLang"/>
		<rdfs:comment xml:lang="en">Java API part implementing the java.nio.charset.spi package for J2SE 1.4</rdfs:comment>
	</owl:Class>
	<owl:Class rdf:about="&j2se-1_4;JavaBeans">
		<rdfs:subClassOf rdf:resource="&j2me-pp-1_1;JavaBeans"/>
		<rdfs:subClassOf rdf:resource="&j2se-1_3;JavaBeans"/>
		<rdfs:seeAlso rdf:resource="&j2se-1_4;JavaAwt"/>
		<rdfs:seeAlso rdf:resource="&j2se-1_4;JavaBeansBeancontext"/>
		<rdfs:seeAlso rdf:resource="&j2se-1_4;JavaApplet"/>
		<rdfs:seeAlso rdf:resource="&j2se-1_4;JavaUtil"/>
		<rdfs:seeAlso rdf:resource="&j2se-1_4;JavaLang"/>
		<rdfs:seeAlso rdf:resource="&j2se-1_4;JavaIo"/>
		<rdfs:seeAlso rdf:resource="&j2se-1_4;JavaLangReflect"/>
		<rdfs:comment xml:lang="en">Java API part implementing the java.beans package for J2SE 1.4</rdfs:comment>
	</owl:Class>
	<owl:Class rdf:about="&j2se-1_4;JavaBeansBeancontext">
		<owl:equivalentClass rdf:resource="&j2se-1_3;JavaBeansBeancontext"/>
		<rdfs:subClassOf rdf:resource="&java;JavaAPIPart"/>
		<rdfs:seeAlso rdf:resource="&j2se-1_4;JavaAwt"/>
		<rdfs:seeAlso rdf:resource="&j2se-1_4;JavaUtil"/>
		<rdfs:seeAlso rdf:resource="&j2se-1_4;JavaLang"/>
		<rdfs:seeAlso rdf:resource="&j2se-1_4;JavaIo"/>
		<rdfs:seeAlso rdf:resource="&j2se-1_4;JavaNet"/>
		<rdfs:seeAlso rdf:resource="&j2se-1_4;JavaBeans"/>
		<rdfs:comment xml:lang="en">Java API part implementing the java.beans.beancontext package for J2SE 1.4</rdfs:comment>
	</owl:Class>
	<owl:Class rdf:about="&j2se-1_4;JavaAwt">
		<rdfs:subClassOf rdf:resource="&j2me-pp-1_1;JavaAwt"/>
		<rdfs:subClassOf rdf:resource="&j2se-1_3;JavaAwt"/>
		<rdfs:seeAlso rdf:resource="&j2se-1_4;JavaLang"/>
		<rdfs:seeAlso rdf:resource="&j2se-1_4;JavaNet"/>
		<rdfs:seeAlso rdf:resource="&j2se-1_4;JavaAwtDnd"/>
		<rdfs:seeAlso rdf:resource="&j2se-1_4;JavaBeans"/>
		<rdfs:seeAlso rdf:resource="&j2se-1_4;JavaAwtEvent"/>
		<rdfs:seeAlso rdf:resource="&j2se-1_4;JavaxSwingText"/>
		<rdfs:seeAlso rdf:resource="&j2se-1_4;JavaSecurity"/>
		<rdfs:seeAlso rdf:resource="&j2se-1_4;JavaUtil"/>
		<rdfs:seeAlso rdf:resource="&j2se-1_4;JavaIo"/>
		<rdfs:seeAlso rdf:resource="&j2se-1_4;JavaText"/>
		<rdfs:seeAlso rdf:resource="&j2se-1_4;JavaAwtGeom"/>
		<rdfs:seeAlso rdf:resource="&j2se-1_4;JavaAwtIm"/>
		<rdfs:seeAlso rdf:resource="&j2se-1_4;JavaAwtDatatransfer"/>
		<rdfs:seeAlso rdf:resource="&j2se-1_4;JavaxAccessibility"/>
		<rdfs:seeAlso rdf:resource="&j2se-1_4;JavaAwtFont"/>
		<rdfs:seeAlso rdf:resource="&j2se-1_4;JavaAwtImageRenderable"/>
		<rdfs:seeAlso rdf:resource="&j2se-1_4;JavaAwtColor"/>
		<rdfs:seeAlso rdf:resource="&j2se-1_4;JavaAwtImage"/>
		<rdfs:comment xml:lang="en">Java API part implementing the java.awt package for J2SE 1.4</rdfs:comment>
	</owl:Class>
	<owl:Class rdf:about="&j2se-1_4;JavaAwtImage">
		<rdfs:subClassOf rdf:resource="&j2me-pp-1_1;JavaAwtImage"/>
		<rdfs:subClassOf rdf:resource="&j2se-1_3;JavaAwtImage"/>
		<rdfs:seeAlso rdf:resource="&j2se-1_4;JavaAwt"/>
		<rdfs:seeAlso rdf:resource="&j2se-1_4;JavaMath"/>
		<rdfs:seeAlso rdf:resource="&j2se-1_4;JavaAwtGeom"/>
		<rdfs:seeAlso rdf:resource="&j2se-1_4;JavaUtil"/>
		<rdfs:seeAlso rdf:resource="&j2se-1_4;JavaLang"/>
		<rdfs:seeAlso rdf:resource="&j2se-1_4;JavaAwtColor"/>
		<rdfs:comment xml:lang="en">Java API part implementing the java.awt.image package for J2SE 1.4</rdfs:comment>
	</owl:Class>
	<owl:Class rdf:about="&j2se-1_4;JavaAwtImageRenderable">
		<owl:equivalentClass rdf:resource="&j2se-1_3;JavaAwtImageRenderable"/>
		<rdfs:subClassOf rdf:resource="&java;JavaAPIPart"/>
		<rdfs:seeAlso rdf:resource="&j2se-1_4;JavaAwt"/>
		<rdfs:seeAlso rdf:resource="&j2se-1_4;JavaAwtGeom"/>
		<rdfs:seeAlso rdf:resource="&j2se-1_4;JavaUtil"/>
		<rdfs:seeAlso rdf:resource="&j2se-1_4;JavaLang"/>
		<rdfs:seeAlso rdf:resource="&j2se-1_4;JavaIo"/>
		<rdfs:seeAlso rdf:resource="&j2se-1_4;JavaAwtImage"/>
		<rdfs:comment xml:lang="en">Java API part implementing the java.awt.image.renderable package for J2SE 1.4</rdfs:comment>
	</owl:Class>
	<owl:Class rdf:about="&j2se-1_4;JavaAwtDatatransfer">
		<rdfs:subClassOf rdf:resource="&j2me-pp-1_1;JavaAwtDatatransfer"/>
		<rdfs:subClassOf rdf:resource="&j2se-1_3;JavaAwtDatatransfer"/>
		<rdfs:seeAlso rdf:resource="&j2se-1_4;JavaUtil"/>
		<rdfs:seeAlso rdf:resource="&j2se-1_4;JavaLang"/>
		<rdfs:seeAlso rdf:resource="&j2se-1_4;JavaIo"/>
		<rdfs:comment xml:lang="en">Java API part implementing the java.awt.datatransfer package for J2SE 1.4</rdfs:comment>
	</owl:Class>
	<owl:Class rdf:about="&j2se-1_4;JavaAwtDnd">
		<rdfs:subClassOf rdf:resource="&j2se-1_3;JavaAwtDnd"/>
		<rdfs:seeAlso rdf:resource="&j2se-1_4;JavaAwtDatatransfer"/>
		<rdfs:seeAlso rdf:resource="&j2se-1_4;JavaAwt"/>
		<rdfs:seeAlso rdf:resource="&j2se-1_4;JavaUtil"/>
		<rdfs:seeAlso rdf:resource="&j2se-1_4;JavaLang"/>
		<rdfs:seeAlso rdf:resource="&j2se-1_4;JavaIo"/>
		<rdfs:seeAlso rdf:resource="&j2se-1_4;JavaAwtEvent"/>
		<rdfs:comment xml:lang="en">Java API part implementing the java.awt.dnd package for J2SE 1.4</rdfs:comment>
	</owl:Class>
	<owl:Class rdf:about="&j2se-1_4;JavaAwtEvent">
		<rdfs:subClassOf rdf:resource="&j2me-pp-1_1;JavaAwtEvent"/>
		<rdfs:subClassOf rdf:resource="&j2se-1_3;JavaAwtEvent"/>
		<rdfs:seeAlso rdf:resource="&j2se-1_4;JavaAwtFont"/>
		<rdfs:seeAlso rdf:resource="&j2se-1_4;JavaText"/>
		<rdfs:seeAlso rdf:resource="&j2se-1_4;JavaAwt"/>
		<rdfs:seeAlso rdf:resource="&j2se-1_4;JavaUtil"/>
		<rdfs:seeAlso rdf:resource="&j2se-1_4;JavaLang"/>
		<rdfs:comment xml:lang="en">Java API part implementing the java.awt.event package for J2SE 1.4</rdfs:comment>
	</owl:Class>
	<owl:Class rdf:about="&j2se-1_4;JavaAwtIm">
		<owl:equivalentClass rdf:resource="&j2se-1_3;JavaAwtIm"/>
		<rdfs:subClassOf rdf:resource="&j2me-pp-1_1;JavaAwtIm"/>
		<rdfs:seeAlso rdf:resource="&j2se-1_4;JavaUtil"/>
		<rdfs:seeAlso rdf:resource="&j2se-1_4;JavaAwtFont"/>
		<rdfs:seeAlso rdf:resource="&j2se-1_4;JavaLang"/>
		<rdfs:seeAlso rdf:resource="&j2se-1_4;JavaText"/>
		<rdfs:seeAlso rdf:resource="&j2se-1_4;JavaAwt"/>
		<rdfs:comment xml:lang="en">Java API part implementing the java.awt.im package for J2SE 1.4</rdfs:comment>
	</owl:Class>
	<owl:Class rdf:about="&j2se-1_4;JavaAwtImSpi">
		<rdfs:subClassOf rdf:resource="&j2se-1_3;JavaAwtImSpi"/>
		<rdfs:seeAlso rdf:resource="&j2se-1_4;JavaAwtIm"/>
		<rdfs:seeAlso rdf:resource="&j2se-1_4;JavaUtil"/>
		<rdfs:seeAlso rdf:resource="&j2se-1_4;JavaAwtFont"/>
		<rdfs:seeAlso rdf:resource="&j2se-1_4;JavaLang"/>
		<rdfs:seeAlso rdf:resource="&j2se-1_4;JavaText"/>
		<rdfs:seeAlso rdf:resource="&j2se-1_4;JavaAwt"/>
		<rdfs:seeAlso rdf:resource="&j2se-1_4;JavaxSwing"/>
		<rdfs:comment xml:lang="en">Java API part implementing the java.awt.im.spi package for J2SE 1.4</rdfs:comment>
	</owl:Class>
	<owl:Class rdf:about="&j2se-1_4;JavaAwtFont">
		<rdfs:subClassOf rdf:resource="&j2me-pp-1_1;JavaAwtFont"/>
		<rdfs:subClassOf rdf:resource="&j2se-1_3;JavaAwtFont"/>
		<rdfs:seeAlso rdf:resource="&j2se-1_4;JavaText"/>
		<rdfs:seeAlso rdf:resource="&j2se-1_4;JavaAwt"/>
		<rdfs:seeAlso rdf:resource="&j2se-1_4;JavaAwtGeom"/>
		<rdfs:seeAlso rdf:resource="&j2se-1_4;JavaUtil"/>
		<rdfs:seeAlso rdf:resource="&j2se-1_4;JavaLang"/>
		<rdfs:seeAlso rdf:resource="&j2se-1_4;JavaIo"/>
		<rdfs:comment xml:lang="en">Java API part implementing the java.awt.font package for J2SE 1.4</rdfs:comment>
	</owl:Class>
	<owl:Class rdf:about="&j2se-1_4;JavaAwtGeom">
		<rdfs:subClassOf rdf:resource="&j2se-1_3;JavaAwtGeom"/>
		<rdfs:seeAlso rdf:resource="&j2se-1_4;JavaLang"/>
		<rdfs:seeAlso rdf:resource="&j2se-1_4;JavaAwt"/>
		<rdfs:seeAlso rdf:resource="&j2se-1_4;JavaIo"/>
		<rdfs:comment xml:lang="en">Java API part implementing the java.awt.geom package for J2SE 1.4</rdfs:comment>
	</owl:Class>
	<owl:Class rdf:about="&j2se-1_4;JavaAwtColor">
		<rdfs:subClassOf rdf:resource="&j2me-pp-1_1;JavaAwtColor"/>
		<rdfs:subClassOf rdf:resource="&j2se-1_3;JavaAwtColor"/>
		<rdfs:seeAlso rdf:resource="&j2se-1_4;JavaLang"/>
		<rdfs:seeAlso rdf:resource="&j2se-1_4;JavaIo"/>
		<rdfs:comment xml:lang="en">Java API part implementing the java.awt.color package for J2SE 1.4</rdfs:comment>
	</owl:Class>
	<owl:Class rdf:about="&j2se-1_4;JavaAwtPrint">
		<rdfs:subClassOf rdf:resource="&j2se-1_3;JavaAwtPrint"/>
		<rdfs:seeAlso rdf:resource="&j2se-1_4;JavaLang"/>
		<rdfs:seeAlso rdf:resource="&j2se-1_4;JavaxPrintAttribute"/>
		<rdfs:seeAlso rdf:resource="&j2se-1_4;JavaAwt"/>
		<rdfs:seeAlso rdf:resource="&j2se-1_4;JavaIo"/>
		<rdfs:seeAlso rdf:resource="&j2se-1_4;JavaxPrint"/>
		<rdfs:comment xml:lang="en">Java API part implementing the java.awt.print package for J2SE 1.4</rdfs:comment>
	</owl:Class>
	<owl:Class rdf:about="&j2se-1_4;JavaText">
		<rdfs:subClassOf rdf:resource="&j2se-1_3;JavaText"/>
		<rdfs:seeAlso rdf:resource="&j2se-1_4;JavaUtil"/>
		<rdfs:seeAlso rdf:resource="&j2se-1_4;JavaLang"/>
		<rdfs:seeAlso rdf:resource="&j2se-1_4;JavaIo"/>
		<rdfs:comment xml:lang="en">Java API part implementing the java.text package for J2SE 1.4</rdfs:comment>
	</owl:Class>
	<owl:Class rdf:about="&j2se-1_4;JavaMath">
		<rdfs:subClassOf rdf:resource="&j2me-pp-1_1;JavaMath"/>
		<rdfs:subClassOf rdf:resource="&j2se-1_3;JavaMath"/>
		<rdfs:seeAlso rdf:resource="&j2se-1_4;JavaUtil"/>
		<rdfs:seeAlso rdf:resource="&j2se-1_4;JavaLang"/>
		<rdfs:comment xml:lang="en">Java API part implementing the java.math package for J2SE 1.4</rdfs:comment>
	</owl:Class>
	<owl:Class rdf:about="&j2se-1_4;JavaApplet">
		<rdfs:subClassOf rdf:resource="&j2me-pp-1_1;JavaApplet"/>
		<rdfs:subClassOf rdf:resource="&j2se-1_3;JavaApplet"/>
		<rdfs:seeAlso rdf:resource="&j2se-1_4;JavaNet"/>
		<rdfs:seeAlso rdf:resource="&j2se-1_4;JavaxAccessibility"/>
		<rdfs:seeAlso rdf:resource="&j2se-1_4;JavaAwt"/>
		<rdfs:seeAlso rdf:resource="&j2se-1_4;JavaUtil"/>
		<rdfs:seeAlso rdf:resource="&j2se-1_4;JavaLang"/>
		<rdfs:seeAlso rdf:resource="&j2se-1_4;JavaIo"/>
		<rdfs:comment xml:lang="en">Java API part implementing the java.applet package for J2SE 1.4</rdfs:comment>
	</owl:Class>
	<owl:Class rdf:about="&j2se-1_4;JavaRmi">
		<rdfs:subClassOf rdf:resource="&j2me-pp-1_1;JavaRmi"/>
		<rdfs:subClassOf rdf:resource="&j2se-1_3;JavaRmi"/>
		<rdfs:seeAlso rdf:resource="&j2se-1_4;JavaLang"/>
		<rdfs:seeAlso rdf:resource="&j2se-1_4;JavaIo"/>
		<rdfs:comment xml:lang="en">Java API part implementing the java.rmi package for J2SE 1.4</rdfs:comment>
	</owl:Class>
	<owl:Class rdf:about="&j2se-1_4;JavaRmiActivation">
		<rdfs:subClassOf rdf:resource="&j2se-1_3;JavaRmiActivation"/>
		<rdfs:seeAlso rdf:resource="&j2se-1_4;JavaRmiServer"/>
		<rdfs:seeAlso rdf:resource="&j2se-1_4;JavaUtil"/>
		<rdfs:seeAlso rdf:resource="&j2se-1_4;JavaLang"/>
		<rdfs:seeAlso rdf:resource="&j2se-1_4;JavaIo"/>
		<rdfs:seeAlso rdf:resource="&j2se-1_4;JavaRmi"/>
		<rdfs:comment xml:lang="en">Java API part implementing the java.rmi.activation package for J2SE 1.4</rdfs:comment>
	</owl:Class>
	<owl:Class rdf:about="&j2se-1_4;JavaRmiServer">
		<rdfs:subClassOf rdf:resource="&j2se-1_3;JavaRmiServer"/>
		<rdfs:seeAlso rdf:resource="&j2se-1_4;JavaNet"/>
		<rdfs:seeAlso rdf:resource="&j2se-1_4;JavaLang"/>
		<rdfs:seeAlso rdf:resource="&j2se-1_4;JavaIo"/>
		<rdfs:seeAlso rdf:resource="&j2se-1_4;JavaLangReflect"/>
		<rdfs:seeAlso rdf:resource="&j2se-1_4;JavaRmi"/>
		<rdfs:comment xml:lang="en">Java API part implementing the java.rmi.server package for J2SE 1.4</rdfs:comment>
	</owl:Class>
	<owl:Class rdf:about="&j2se-1_4;JavaRmiDgc">
		<owl:equivalentClass rdf:resource="&j2se-1_3;JavaRmiDgc"/>
		<rdfs:subClassOf rdf:resource="&java;JavaAPIPart"/>
		<rdfs:seeAlso rdf:resource="&j2se-1_4;JavaLang"/>
		<rdfs:seeAlso rdf:resource="&j2se-1_4;JavaIo"/>
		<rdfs:seeAlso rdf:resource="&j2se-1_4;JavaRmi"/>
		<rdfs:comment xml:lang="en">Java API part implementing the java.rmi.dgc package for J2SE 1.4</rdfs:comment>
	</owl:Class>
	<owl:Class rdf:about="&j2se-1_4;JavaRmiRegistry">
		<owl:equivalentClass rdf:resource="&j2se-1_3;JavaRmiRegistry"/>
		<rdfs:subClassOf rdf:resource="&j2me-pp-1_1;JavaRmiRegistry"/>
		<rdfs:seeAlso rdf:resource="&j2se-1_4;JavaRmiServer"/>
		<rdfs:seeAlso rdf:resource="&j2se-1_4;JavaLang"/>
		<rdfs:seeAlso rdf:resource="&j2se-1_4;JavaRmi"/>
		<rdfs:comment xml:lang="en">Java API part implementing the java.rmi.registry package for J2SE 1.4</rdfs:comment>
	</owl:Class>
	<owl:Class rdf:about="&j2se-1_4;JavaSql">
		<rdfs:subClassOf rdf:resource="&j2se-1_3;JavaSql"/>
		<rdfs:seeAlso rdf:resource="&j2se-1_4;JavaNet"/>
		<rdfs:seeAlso rdf:resource="&j2se-1_4;JavaMath"/>
		<rdfs:seeAlso rdf:resource="&j2se-1_4;JavaSecurity"/>
		<rdfs:seeAlso rdf:resource="&j2se-1_4;JavaUtil"/>
		<rdfs:seeAlso rdf:resource="&j2se-1_4;JavaLang"/>
		<rdfs:seeAlso rdf:resource="&j2se-1_4;JavaIo"/>
		<rdfs:comment xml:lang="en">Java API part implementing the java.sql package for J2SE 1.4</rdfs:comment>
	</owl:Class>
	<owl:Class rdf:about="&j2se-1_4;JavaxImageio">
		<rdfs:subClassOf rdf:resource="&java;JavaAPIPart"/>
		<rdfs:seeAlso rdf:resource="&j2se-1_4;JavaAwt"/>
		<rdfs:seeAlso rdf:resource="&j2se-1_4;JavaUtil"/>
		<rdfs:seeAlso rdf:resource="&j2se-1_4;JavaLang"/>
		<rdfs:seeAlso rdf:resource="&j2se-1_4;JavaIo"/>
		<rdfs:seeAlso rdf:resource="&j2se-1_4;JavaxImageioMetadata"/>
		<rdfs:seeAlso rdf:resource="&j2se-1_4;JavaNet"/>
		<rdfs:seeAlso rdf:resource="&j2se-1_4;JavaxImageioEvent"/>
		<rdfs:seeAlso rdf:resource="&j2se-1_4;JavaxImageioStream"/>
		<rdfs:seeAlso rdf:resource="&j2se-1_4;JavaxImageioSpi"/>
		<rdfs:seeAlso rdf:resource="&j2se-1_4;JavaAwtColor"/>
		<rdfs:seeAlso rdf:resource="&j2se-1_4;JavaAwtImage"/>
		<rdfs:comment xml:lang="en">Java API part implementing the javax.imageio package for J2SE 1.4</rdfs:comment>
	</owl:Class>
	<owl:Class rdf:about="&j2se-1_4;JavaxImageioSpi">
		<rdfs:subClassOf rdf:resource="&java;JavaAPIPart"/>
		<rdfs:seeAlso rdf:resource="&j2se-1_4;JavaxImageioStream"/>
		<rdfs:seeAlso rdf:resource="&j2se-1_4;JavaxImageio"/>
		<rdfs:seeAlso rdf:resource="&j2se-1_4;JavaUtil"/>
		<rdfs:seeAlso rdf:resource="&j2se-1_4;JavaLang"/>
		<rdfs:seeAlso rdf:resource="&j2se-1_4;JavaIo"/>
		<rdfs:seeAlso rdf:resource="&j2se-1_4;JavaAwtImage"/>
		<rdfs:seeAlso rdf:resource="&j2se-1_4;JavaxImageioMetadata"/>
		<rdfs:comment xml:lang="en">Java API part implementing the javax.imageio.spi package for J2SE 1.4</rdfs:comment>
	</owl:Class>
	<owl:Class rdf:about="&j2se-1_4;JavaxImageioMetadata">
		<rdfs:subClassOf rdf:resource="&java;JavaAPIPart"/>
		<rdfs:seeAlso rdf:resource="&j2se-1_4;JavaxImageio"/>
		<rdfs:seeAlso rdf:resource="&j2se-1_4;OrgW3cDom"/>
		<rdfs:seeAlso rdf:resource="&j2se-1_4;JavaUtil"/>
		<rdfs:seeAlso rdf:resource="&j2se-1_4;JavaLang"/>
		<rdfs:comment xml:lang="en">Java API part implementing the javax.imageio.metadata package for J2SE 1.4</rdfs:comment>
	</owl:Class>
	<owl:Class rdf:about="&j2se-1_4;JavaxImageioStream">
		<rdfs:subClassOf rdf:resource="&java;JavaAPIPart"/>
		<rdfs:seeAlso rdf:resource="&j2se-1_4;JavaLang"/>
		<rdfs:seeAlso rdf:resource="&j2se-1_4;JavaIo"/>
		<rdfs:seeAlso rdf:resource="&j2se-1_4;JavaNio"/>
		<rdfs:comment xml:lang="en">Java API part implementing the javax.imageio.stream package for J2SE 1.4</rdfs:comment>
	</owl:Class>
	<owl:Class rdf:about="&j2se-1_4;JavaxImageioEvent">
		<rdfs:subClassOf rdf:resource="&java;JavaAPIPart"/>
		<rdfs:seeAlso rdf:resource="&j2se-1_4;JavaUtil"/>
		<rdfs:seeAlso rdf:resource="&j2se-1_4;JavaLang"/>
		<rdfs:seeAlso rdf:resource="&j2se-1_4;JavaxImageio"/>
		<rdfs:seeAlso rdf:resource="&j2se-1_4;JavaAwtImage"/>
		<rdfs:comment xml:lang="en">Java API part implementing the javax.imageio.event package for J2SE 1.4</rdfs:comment>
	</owl:Class>
	<owl:Class rdf:about="&j2se-1_4;JavaxImageioPluginsJpeg">
		<rdfs:subClassOf rdf:resource="&java;JavaAPIPart"/>
		<rdfs:seeAlso rdf:resource="&j2se-1_4;JavaUtil"/>
		<rdfs:seeAlso rdf:resource="&j2se-1_4;JavaLang"/>
		<rdfs:seeAlso rdf:resource="&j2se-1_4;JavaxImageio"/>
		<rdfs:comment xml:lang="en">Java API part implementing the javax.imageio.plugins.jpeg package for J2SE 1.4</rdfs:comment>
	</owl:Class>
	<owl:Class rdf:about="&j2se-1_4;JavaxAccessibility">
		<rdfs:subClassOf rdf:resource="&j2se-1_3;JavaxAccessibility"/>
		<rdfs:seeAlso rdf:resource="&j2se-1_4;JavaBeans"/>
		<rdfs:seeAlso rdf:resource="&j2se-1_4;JavaAwt"/>
		<rdfs:seeAlso rdf:resource="&j2se-1_4;JavaxSwingText"/>
		<rdfs:seeAlso rdf:resource="&j2se-1_4;JavaUtil"/>
		<rdfs:seeAlso rdf:resource="&j2se-1_4;JavaAwtEvent"/>
		<rdfs:seeAlso rdf:resource="&j2se-1_4;JavaLang"/>
		<rdfs:comment xml:lang="en">Java API part implementing the javax.accessibility package for J2SE 1.4</rdfs:comment>
	</owl:Class>
	<owl:Class rdf:about="&j2se-1_4;JavaxSwing">
		<rdfs:subClassOf rdf:resource="&java;JavaAPIPart"/>
		<rdfs:seeAlso rdf:resource="&j2se-1_4;JavaAwt"/>
		<rdfs:seeAlso rdf:resource="&j2se-1_4;JavaNet"/>
		<rdfs:seeAlso rdf:resource="&j2se-1_4;JavaAwtEvent"/>
		<rdfs:seeAlso rdf:resource="&j2se-1_4;JavaUtil"/>
		<rdfs:seeAlso rdf:resource="&j2se-1_4;JavaxSwingPlaf"/>
		<rdfs:seeAlso rdf:resource="&j2se-1_4;JavaIo"/>
		<rdfs:seeAlso rdf:resource="&j2se-1_4;JavaAwtDatatransfer"/>
		<rdfs:seeAlso rdf:resource="&j2se-1_4;JavaxSwingEvent"/>
		<rdfs:seeAlso rdf:resource="&j2se-1_4;JavaxAccessibility"/>
		<rdfs:seeAlso rdf:resource="&j2se-1_4;JavaxSwingFilechooser"/>
		<rdfs:seeAlso rdf:resource="&j2se-1_4;JavaApplet"/>
		<rdfs:seeAlso rdf:resource="&j2se-1_4;JavaxSwingTable"/>
		<rdfs:seeAlso rdf:resource="&j2se-1_4;JavaLang"/>
		<rdfs:seeAlso rdf:resource="&j2se-1_4;JavaxSwingColorchooser"/>
		<rdfs:seeAlso rdf:resource="&j2se-1_4;JavaBeans"/>
		<rdfs:seeAlso rdf:resource="&j2se-1_4;JavaxSwingText"/>
		<rdfs:seeAlso rdf:resource="&j2se-1_4;JavaText"/>
		<rdfs:seeAlso rdf:resource="&j2se-1_4;JavaxSwingBorder"/>
		<rdfs:seeAlso rdf:resource="&j2se-1_4;JavaxSwingTree"/>
		<rdfs:seeAlso rdf:resource="&j2se-1_4;JavaAwtImage"/>
		<rdfs:comment xml:lang="en">Java API part implementing the javax.swing package for J2SE 1.4</rdfs:comment>
	</owl:Class>
	<owl:Class rdf:about="&j2se-1_4;JavaxSwingPlaf">
		<rdfs:subClassOf rdf:resource="&j2se-1_3;JavaxSwingPlaf"/>
		<rdfs:seeAlso rdf:resource="&j2se-1_4;JavaAwt"/>
		<rdfs:seeAlso rdf:resource="&j2se-1_4;JavaxSwingText"/>
		<rdfs:seeAlso rdf:resource="&j2se-1_4;JavaLang"/>
		<rdfs:seeAlso rdf:resource="&j2se-1_4;JavaIo"/>
		<rdfs:seeAlso rdf:resource="&j2se-1_4;JavaxSwingBorder"/>
		<rdfs:seeAlso rdf:resource="&j2se-1_4;JavaxAccessibility"/>
		<rdfs:seeAlso rdf:resource="&j2se-1_4;JavaxSwing"/>
		<rdfs:seeAlso rdf:resource="&j2se-1_4;JavaAwtEvent"/>
		<rdfs:seeAlso rdf:resource="&j2se-1_4;JavaxSwingTree"/>
		<rdfs:seeAlso rdf:resource="&j2se-1_4;JavaxSwingFilechooser"/>
		<rdfs:comment xml:lang="en">Java API part implementing the javax.swing.plaf package for J2SE 1.4</rdfs:comment>
	</owl:Class>
	<owl:Class rdf:about="&j2se-1_4;JavaxSwingPlafBasic">
		<rdfs:subClassOf rdf:resource="&j2se-1_3;JavaxSwingPlafBasic"/>
		<rdfs:seeAlso rdf:resource="&j2se-1_4;JavaAwt"/>
		<rdfs:seeAlso rdf:resource="&j2se-1_4;JavaxSwingTable"/>
		<rdfs:seeAlso rdf:resource="&j2se-1_4;JavaLang"/>
		<rdfs:seeAlso rdf:resource="&j2se-1_4;JavaBeans"/>
		<rdfs:seeAlso rdf:resource="&j2se-1_4;JavaAwtEvent"/>
		<rdfs:seeAlso rdf:resource="&j2se-1_4;JavaxSwingText"/>
		<rdfs:seeAlso rdf:resource="&j2se-1_4;JavaUtil"/>
		<rdfs:seeAlso rdf:resource="&j2se-1_4;JavaxSwingPlaf"/>
		<rdfs:seeAlso rdf:resource="&j2se-1_4;JavaIo"/>
		<rdfs:seeAlso rdf:resource="&j2se-1_4;JavaxSwingEvent"/>
		<rdfs:seeAlso rdf:resource="&j2se-1_4;JavaxSwingBorder"/>
		<rdfs:seeAlso rdf:resource="&j2se-1_4;JavaxAccessibility"/>
		<rdfs:seeAlso rdf:resource="&j2se-1_4;JavaxSwing"/>
		<rdfs:seeAlso rdf:resource="&j2se-1_4;JavaxSwingTree"/>
		<rdfs:seeAlso rdf:resource="&j2se-1_4;JavaxSwingFilechooser"/>
		<rdfs:comment xml:lang="en">Java API part implementing the javax.swing.plaf.basic package for J2SE 1.4</rdfs:comment>
	</owl:Class>
	<owl:Class rdf:about="&j2se-1_4;JavaxSwingPlafMetal">
		<rdfs:subClassOf rdf:resource="&j2se-1_3;JavaxSwingPlafMetal"/>
		<rdfs:seeAlso rdf:resource="&j2se-1_4;JavaAwt"/>
		<rdfs:seeAlso rdf:resource="&j2se-1_4;JavaLang"/>
		<rdfs:seeAlso rdf:resource="&j2se-1_4;JavaxSwingPlafBasic"/>
		<rdfs:seeAlso rdf:resource="&j2se-1_4;JavaxSwingEvent"/>
		<rdfs:seeAlso rdf:resource="&j2se-1_4;JavaxSwingBorder"/>
		<rdfs:seeAlso rdf:resource="&j2se-1_4;JavaBeans"/>
		<rdfs:seeAlso rdf:resource="&j2se-1_4;JavaxSwing"/>
		<rdfs:seeAlso rdf:resource="&j2se-1_4;JavaAwtEvent"/>
		<rdfs:seeAlso rdf:resource="&j2se-1_4;JavaxSwingTree"/>
		<rdfs:seeAlso rdf:resource="&j2se-1_4;JavaxSwingPlaf"/>
		<rdfs:seeAlso rdf:resource="&j2se-1_4;JavaIo"/>
		<rdfs:comment xml:lang="en">Java API part implementing the javax.swing.plaf.metal package for J2SE 1.4</rdfs:comment>
	</owl:Class>
	<owl:Class rdf:about="&j2se-1_4;JavaxSwingPlafMulti">
		<rdfs:subClassOf rdf:resource="&j2se-1_3;JavaxSwingPlafMulti"/>
		<rdfs:seeAlso rdf:resource="&j2se-1_4;JavaAwt"/>
		<rdfs:seeAlso rdf:resource="&j2se-1_4;JavaLang"/>
		<rdfs:seeAlso rdf:resource="&j2se-1_4;JavaxAccessibility"/>
		<rdfs:seeAlso rdf:resource="&j2se-1_4;JavaxSwing"/>
		<rdfs:seeAlso rdf:resource="&j2se-1_4;JavaAwtEvent"/>
		<rdfs:seeAlso rdf:resource="&j2se-1_4;JavaxSwingTree"/>
		<rdfs:seeAlso rdf:resource="&j2se-1_4;JavaxSwingFilechooser"/>
		<rdfs:seeAlso rdf:resource="&j2se-1_4;JavaxSwingText"/>
		<rdfs:seeAlso rdf:resource="&j2se-1_4;JavaUtil"/>
		<rdfs:seeAlso rdf:resource="&j2se-1_4;JavaxSwingPlaf"/>
		<rdfs:seeAlso rdf:resource="&j2se-1_4;JavaIo"/>
		<rdfs:comment xml:lang="en">Java API part implementing the javax.swing.plaf.multi package for J2SE 1.4</rdfs:comment>
	</owl:Class>
	<owl:Class rdf:about="&j2se-1_4;JavaxSwingEvent">
		<rdfs:subClassOf rdf:resource="&j2se-1_3;JavaxSwingEvent"/>
		<rdfs:seeAlso rdf:resource="&j2se-1_4;JavaxSwingUndo"/>
		<rdfs:seeAlso rdf:resource="&j2se-1_4;JavaAwt"/>
		<rdfs:seeAlso rdf:resource="&j2se-1_4;JavaxSwingText"/>
		<rdfs:seeAlso rdf:resource="&j2se-1_4;JavaUtil"/>
		<rdfs:seeAlso rdf:resource="&j2se-1_4;JavaxSwingTable"/>
		<rdfs:seeAlso rdf:resource="&j2se-1_4;JavaLang"/>
		<rdfs:seeAlso rdf:resource="&j2se-1_4;JavaIo"/>
		<rdfs:seeAlso rdf:resource="&j2se-1_4;JavaNet"/>
		<rdfs:seeAlso rdf:resource="&j2se-1_4;JavaBeans"/>
		<rdfs:seeAlso rdf:resource="&j2se-1_4;JavaxSwing"/>
		<rdfs:seeAlso rdf:resource="&j2se-1_4;JavaAwtEvent"/>
		<rdfs:seeAlso rdf:resource="&j2se-1_4;JavaxSwingTree"/>
		<rdfs:comment xml:lang="en">Java API part implementing the javax.swing.event package for J2SE 1.4</rdfs:comment>
	</owl:Class>
	<owl:Class rdf:about="&j2se-1_4;JavaxSwingBorder">
		<owl:equivalentClass rdf:resource="&j2se-1_3;JavaxSwingBorder"/>
		<rdfs:subClassOf rdf:resource="&java;JavaAPIPart"/>
		<rdfs:seeAlso rdf:resource="&j2se-1_4;JavaLang"/>
		<rdfs:seeAlso rdf:resource="&j2se-1_4;JavaAwt"/>
		<rdfs:seeAlso rdf:resource="&j2se-1_4;JavaIo"/>
		<rdfs:seeAlso rdf:resource="&j2se-1_4;JavaxSwing"/>
		<rdfs:comment xml:lang="en">Java API part implementing the javax.swing.border package for J2SE 1.4</rdfs:comment>
	</owl:Class>
	<owl:Class rdf:about="&j2se-1_4;JavaxSwingText">
		<rdfs:subClassOf rdf:resource="&j2se-1_3;JavaxSwingText"/>
		<rdfs:seeAlso rdf:resource="&j2se-1_4;JavaAwt"/>
		<rdfs:seeAlso rdf:resource="&j2se-1_4;JavaLang"/>
		<rdfs:seeAlso rdf:resource="&j2se-1_4;JavaxSwingPlafBasic"/>
		<rdfs:seeAlso rdf:resource="&j2se-1_4;JavaxSwingEvent"/>
		<rdfs:seeAlso rdf:resource="&j2se-1_4;JavaxAccessibility"/>
		<rdfs:seeAlso rdf:resource="&j2se-1_4;JavaxSwing"/>
		<rdfs:seeAlso rdf:resource="&j2se-1_4;JavaAwtEvent"/>
		<rdfs:seeAlso rdf:resource="&j2se-1_4;JavaxSwingTree"/>
		<rdfs:seeAlso rdf:resource="&j2se-1_4;JavaxSwingUndo"/>
		<rdfs:seeAlso rdf:resource="&j2se-1_4;JavaUtil"/>
		<rdfs:seeAlso rdf:resource="&j2se-1_4;JavaxSwingPlaf"/>
		<rdfs:seeAlso rdf:resource="&j2se-1_4;JavaIo"/>
		<rdfs:seeAlso rdf:resource="&j2se-1_4;JavaText"/>
		<rdfs:seeAlso rdf:resource="&j2se-1_4;JavaAwtIm"/>
		<rdfs:comment xml:lang="en">Java API part implementing the javax.swing.text package for J2SE 1.4</rdfs:comment>
	</owl:Class>
	<owl:Class rdf:about="&j2se-1_4;JavaxSwingTextHtml">
		<rdfs:subClassOf rdf:resource="&j2se-1_3;JavaxSwingTextHtml"/>
		<rdfs:seeAlso rdf:resource="&j2se-1_4;JavaAwt"/>
		<rdfs:seeAlso rdf:resource="&j2se-1_4;JavaLang"/>
		<rdfs:seeAlso rdf:resource="&j2se-1_4;JavaNet"/>
		<rdfs:seeAlso rdf:resource="&j2se-1_4;JavaxSwingEvent"/>
		<rdfs:seeAlso rdf:resource="&j2se-1_4;JavaxAccessibility"/>
		<rdfs:seeAlso rdf:resource="&j2se-1_4;JavaxSwing"/>
		<rdfs:seeAlso rdf:resource="&j2se-1_4;JavaAwtEvent"/>
		<rdfs:seeAlso rdf:resource="&j2se-1_4;JavaxSwingText"/>
		<rdfs:seeAlso rdf:resource="&j2se-1_4;JavaUtil"/>
		<rdfs:seeAlso rdf:resource="&j2se-1_4;JavaIo"/>
		<rdfs:comment xml:lang="en">Java API part implementing the javax.swing.text.html package for J2SE 1.4</rdfs:comment>
	</owl:Class>
	<owl:Class rdf:about="&j2se-1_4;JavaxSwingTextHtmlParser">
		<owl:equivalentClass rdf:resource="&j2se-1_3;JavaxSwingTextHtmlParser"/>
		<rdfs:subClassOf rdf:resource="&java;JavaAPIPart"/>
		<rdfs:seeAlso rdf:resource="&j2se-1_4;JavaxSwingTextHtml"/>
		<rdfs:seeAlso rdf:resource="&j2se-1_4;JavaxSwingText"/>
		<rdfs:seeAlso rdf:resource="&j2se-1_4;JavaUtil"/>
		<rdfs:seeAlso rdf:resource="&j2se-1_4;JavaLang"/>
		<rdfs:seeAlso rdf:resource="&j2se-1_4;JavaIo"/>
		<rdfs:comment xml:lang="en">Java API part implementing the javax.swing.text.html.parser package for J2SE 1.4</rdfs:comment>
	</owl:Class>
	<owl:Class rdf:about="&j2se-1_4;JavaxSwingTextRtf">
		<owl:equivalentClass rdf:resource="&j2se-1_3;JavaxSwingTextRtf"/>
		<rdfs:subClassOf rdf:resource="&java;JavaAPIPart"/>
		<rdfs:seeAlso rdf:resource="&j2se-1_4;JavaLang"/>
		<rdfs:seeAlso rdf:resource="&j2se-1_4;JavaIo"/>
		<rdfs:seeAlso rdf:resource="&j2se-1_4;JavaxSwingText"/>
		<rdfs:comment xml:lang="en">Java API part implementing the javax.swing.text.rtf package for J2SE 1.4</rdfs:comment>
	</owl:Class>
	<owl:Class rdf:about="&j2se-1_4;JavaxSwingTable">
		<rdfs:subClassOf rdf:resource="&j2se-1_3;JavaxSwingTable"/>
		<rdfs:seeAlso rdf:resource="&j2se-1_4;JavaAwt"/>
		<rdfs:seeAlso rdf:resource="&j2se-1_4;JavaUtil"/>
		<rdfs:seeAlso rdf:resource="&j2se-1_4;JavaLang"/>
		<rdfs:seeAlso rdf:resource="&j2se-1_4;JavaxSwingPlaf"/>
		<rdfs:seeAlso rdf:resource="&j2se-1_4;JavaIo"/>
		<rdfs:seeAlso rdf:resource="&j2se-1_4;JavaxSwingEvent"/>
		<rdfs:seeAlso rdf:resource="&j2se-1_4;JavaxSwingBorder"/>
		<rdfs:seeAlso rdf:resource="&j2se-1_4;JavaBeans"/>
		<rdfs:seeAlso rdf:resource="&j2se-1_4;JavaxAccessibility"/>
		<rdfs:seeAlso rdf:resource="&j2se-1_4;JavaxSwing"/>
		<rdfs:seeAlso rdf:resource="&j2se-1_4;JavaAwtEvent"/>
		<rdfs:comment xml:lang="en">Java API part implementing the javax.swing.table package for J2SE 1.4</rdfs:comment>
	</owl:Class>
	<owl:Class rdf:about="&j2se-1_4;JavaxSwingUndo">
		<rdfs:subClassOf rdf:resource="&j2se-1_3;JavaxSwingUndo"/>
		<rdfs:seeAlso rdf:resource="&j2se-1_4;JavaUtil"/>
		<rdfs:seeAlso rdf:resource="&j2se-1_4;JavaxSwingEvent"/>
		<rdfs:seeAlso rdf:resource="&j2se-1_4;JavaLang"/>
		<rdfs:seeAlso rdf:resource="&j2se-1_4;JavaIo"/>
		<rdfs:comment xml:lang="en">Java API part implementing the javax.swing.undo package for J2SE 1.4</rdfs:comment>
	</owl:Class>
	<owl:Class rdf:about="&j2se-1_4;JavaxSwingTree">
		<rdfs:subClassOf rdf:resource="&j2se-1_3;JavaxSwingTree"/>
		<rdfs:seeAlso rdf:resource="&j2se-1_4;JavaAwt"/>
		<rdfs:seeAlso rdf:resource="&j2se-1_4;JavaUtil"/>
		<rdfs:seeAlso rdf:resource="&j2se-1_4;JavaLang"/>
		<rdfs:seeAlso rdf:resource="&j2se-1_4;JavaIo"/>
		<rdfs:seeAlso rdf:resource="&j2se-1_4;JavaxSwingEvent"/>
		<rdfs:seeAlso rdf:resource="&j2se-1_4;JavaxSwingBorder"/>
		<rdfs:seeAlso rdf:resource="&j2se-1_4;JavaBeans"/>
		<rdfs:seeAlso rdf:resource="&j2se-1_4;JavaxSwing"/>
		<rdfs:seeAlso rdf:resource="&j2se-1_4;JavaAwtEvent"/>
		<rdfs:comment xml:lang="en">Java API part implementing the javax.swing.tree package for J2SE 1.4</rdfs:comment>
	</owl:Class>
	<owl:Class rdf:about="&j2se-1_4;JavaxSwingFilechooser">
		<rdfs:subClassOf rdf:resource="&j2se-1_3;JavaxSwingFilechooser"/>
		<rdfs:seeAlso rdf:resource="&j2se-1_4;JavaLang"/>
		<rdfs:seeAlso rdf:resource="&j2se-1_4;JavaIo"/>
		<rdfs:seeAlso rdf:resource="&j2se-1_4;JavaxSwing"/>
		<rdfs:comment xml:lang="en">Java API part implementing the javax.swing.filechooser package for J2SE 1.4</rdfs:comment>
	</owl:Class>
	<owl:Class rdf:about="&j2se-1_4;JavaxSwingColorchooser">
		<rdfs:subClassOf rdf:resource="&j2se-1_3;JavaxSwingColorchooser"/>
		<rdfs:seeAlso rdf:resource="&j2se-1_4;JavaxSwingEvent"/>
		<rdfs:seeAlso rdf:resource="&j2se-1_4;JavaAwt"/>
		<rdfs:seeAlso rdf:resource="&j2se-1_4;JavaxSwing"/>
		<rdfs:seeAlso rdf:resource="&j2se-1_4;JavaLang"/>
		<rdfs:seeAlso rdf:resource="&j2se-1_4;JavaIo"/>
		<rdfs:comment xml:lang="en">Java API part implementing the javax.swing.colorchooser package for J2SE 1.4</rdfs:comment>
	</owl:Class>
	<owl:Class rdf:about="&j2se-1_4;JavaxSoundSampled">
		<rdfs:subClassOf rdf:resource="&j2se-1_3;JavaxSoundSampled"/>
		<rdfs:seeAlso rdf:resource="&j2se-1_4;JavaNet"/>
		<rdfs:seeAlso rdf:resource="&j2se-1_4;JavaSecurity"/>
		<rdfs:seeAlso rdf:resource="&j2se-1_4;JavaUtil"/>
		<rdfs:seeAlso rdf:resource="&j2se-1_4;JavaLang"/>
		<rdfs:seeAlso rdf:resource="&j2se-1_4;JavaIo"/>
		<rdfs:comment xml:lang="en">Java API part implementing the javax.sound.sampled package for J2SE 1.4</rdfs:comment>
	</owl:Class>
	<owl:Class rdf:about="&j2se-1_4;JavaxSoundSampledSpi">
		<owl:equivalentClass rdf:resource="&j2se-1_3;JavaxSoundSampledSpi"/>
		<rdfs:subClassOf rdf:resource="&java;JavaAPIPart"/>
		<rdfs:seeAlso rdf:resource="&j2se-1_4;JavaNet"/>
		<rdfs:seeAlso rdf:resource="&j2se-1_4;JavaxSoundSampled"/>
		<rdfs:seeAlso rdf:resource="&j2se-1_4;JavaLang"/>
		<rdfs:seeAlso rdf:resource="&j2se-1_4;JavaIo"/>
		<rdfs:comment xml:lang="en">Java API part implementing the javax.sound.sampled.spi package for J2SE 1.4</rdfs:comment>
	</owl:Class>
	<owl:Class rdf:about="&j2se-1_4;JavaxSoundMidi">
		<rdfs:subClassOf rdf:resource="&j2se-1_3;JavaxSoundMidi"/>
		<rdfs:seeAlso rdf:resource="&j2se-1_4;JavaNet"/>
		<rdfs:seeAlso rdf:resource="&j2se-1_4;JavaUtil"/>
		<rdfs:seeAlso rdf:resource="&j2se-1_4;JavaLang"/>
		<rdfs:seeAlso rdf:resource="&j2se-1_4;JavaIo"/>
		<rdfs:comment xml:lang="en">Java API part implementing the javax.sound.midi package for J2SE 1.4</rdfs:comment>
	</owl:Class>
	<owl:Class rdf:about="&j2se-1_4;JavaxSoundMidiSpi">
		<owl:equivalentClass rdf:resource="&j2se-1_3;JavaxSoundMidiSpi"/>
		<rdfs:subClassOf rdf:resource="&java;JavaAPIPart"/>
		<rdfs:seeAlso rdf:resource="&j2se-1_4;JavaNet"/>
		<rdfs:seeAlso rdf:resource="&j2se-1_4;JavaLang"/>
		<rdfs:seeAlso rdf:resource="&j2se-1_4;JavaIo"/>
		<rdfs:seeAlso rdf:resource="&j2se-1_4;JavaxSoundMidi"/>
		<rdfs:comment xml:lang="en">Java API part implementing the javax.sound.midi.spi package for J2SE 1.4</rdfs:comment>
	</owl:Class>
	<owl:Class rdf:about="&j2se-1_4;JavaxPrint">
		<rdfs:subClassOf rdf:resource="&java;JavaAPIPart"/>
		<rdfs:seeAlso rdf:resource="&j2se-1_4;JavaNet"/>
		<rdfs:seeAlso rdf:resource="&j2se-1_4;JavaxPrintEvent"/>
		<rdfs:seeAlso rdf:resource="&j2se-1_4;JavaAwt"/>
		<rdfs:seeAlso rdf:resource="&j2se-1_4;JavaxPrintAttribute"/>
		<rdfs:seeAlso rdf:resource="&j2se-1_4;JavaLang"/>
		<rdfs:seeAlso rdf:resource="&j2se-1_4;JavaIo"/>
		<rdfs:comment xml:lang="en">Java API part implementing the javax.print package for J2SE 1.4</rdfs:comment>
	</owl:Class>
	<owl:Class rdf:about="&j2se-1_4;JavaxPrintAttribute">
		<rdfs:subClassOf rdf:resource="&java;JavaAPIPart"/>
		<rdfs:seeAlso rdf:resource="&j2se-1_4;JavaNet"/>
		<rdfs:seeAlso rdf:resource="&j2se-1_4;JavaUtil"/>
		<rdfs:seeAlso rdf:resource="&j2se-1_4;JavaLang"/>
		<rdfs:seeAlso rdf:resource="&j2se-1_4;JavaIo"/>
		<rdfs:comment xml:lang="en">Java API part implementing the javax.print.attribute package for J2SE 1.4</rdfs:comment>
	</owl:Class>
	<owl:Class rdf:about="&j2se-1_4;JavaxPrintAttributeStandard">
		<rdfs:subClassOf rdf:resource="&java;JavaAPIPart"/>
		<rdfs:seeAlso rdf:resource="&j2se-1_4;JavaUtil"/>
		<rdfs:seeAlso rdf:resource="&j2se-1_4;JavaLang"/>
		<rdfs:seeAlso rdf:resource="&j2se-1_4;JavaNet"/>
		<rdfs:seeAlso rdf:resource="&j2se-1_4;JavaxPrintAttribute"/>
		<rdfs:comment xml:lang="en">Java API part implementing the javax.print.attribute.standard package for J2SE 1.4</rdfs:comment>
	</owl:Class>
	<owl:Class rdf:about="&j2se-1_4;JavaxPrintEvent">
		<rdfs:subClassOf rdf:resource="&java;JavaAPIPart"/>
		<rdfs:seeAlso rdf:resource="&j2se-1_4;JavaUtil"/>
		<rdfs:seeAlso rdf:resource="&j2se-1_4;JavaLang"/>
		<rdfs:seeAlso rdf:resource="&j2se-1_4;JavaxPrintAttribute"/>
		<rdfs:seeAlso rdf:resource="&j2se-1_4;JavaxPrint"/>
		<rdfs:comment xml:lang="en">Java API part implementing the javax.print.event package for J2SE 1.4</rdfs:comment>
	</owl:Class>
	<owl:Class rdf:about="&j2se-1_4;JavaxSecurityAuth">
		<rdfs:subClassOf rdf:resource="&java;JavaAPIPart"/>
		<rdfs:seeAlso rdf:resource="&j2se-1_4;JavaUtil"/>
		<rdfs:seeAlso rdf:resource="&j2se-1_4;JavaSecurity"/>
		<rdfs:seeAlso rdf:resource="&j2se-1_4;JavaLang"/>
		<rdfs:seeAlso rdf:resource="&j2se-1_4;JavaIo"/>
		<rdfs:comment xml:lang="en">Java API part implementing the javax.security.auth package for J2SE 1.4</rdfs:comment>
	</owl:Class>
	<owl:Class rdf:about="&j2se-1_4;JavaxSecurityAuthX500">
		<rdfs:subClassOf rdf:resource="&j2me-pp-1_1;JavaxSecurityAuthX500"/>
		<rdfs:seeAlso rdf:resource="&j2se-1_4;JavaSecurity"/>
		<rdfs:seeAlso rdf:resource="&j2se-1_4;JavaLang"/>
		<rdfs:seeAlso rdf:resource="&j2se-1_4;JavaSecurityCert"/>
		<rdfs:seeAlso rdf:resource="&j2se-1_4;JavaIo"/>
		<rdfs:seeAlso rdf:resource="&j2se-1_4;JavaxSecurityAuth"/>
		<rdfs:comment xml:lang="en">Java API part implementing the javax.security.auth.x500 package for J2SE 1.4</rdfs:comment>
	</owl:Class>
	<owl:Class rdf:about="&j2se-1_4;JavaxSecurityAuthCallback">
		<rdfs:subClassOf rdf:resource="&java;JavaAPIPart"/>
		<rdfs:seeAlso rdf:resource="&j2se-1_4;JavaUtil"/>
		<rdfs:seeAlso rdf:resource="&j2se-1_4;JavaLang"/>
		<rdfs:seeAlso rdf:resource="&j2se-1_4;JavaIo"/>
		<rdfs:comment xml:lang="en">Java API part implementing the javax.security.auth.callback package for J2SE 1.4</rdfs:comment>
	</owl:Class>
	<owl:Class rdf:about="&j2se-1_4;JavaxSecurityAuthKerberos">
		<rdfs:subClassOf rdf:resource="&java;JavaAPIPart"/>
		<rdfs:seeAlso rdf:resource="&j2se-1_4;JavaUtil"/>
		<rdfs:seeAlso rdf:resource="&j2se-1_4;JavaSecurity"/>
		<rdfs:seeAlso rdf:resource="&j2se-1_4;JavaLang"/>
		<rdfs:seeAlso rdf:resource="&j2se-1_4;JavaxCrypto"/>
		<rdfs:seeAlso rdf:resource="&j2se-1_4;JavaIo"/>
		<rdfs:seeAlso rdf:resource="&j2se-1_4;JavaxSecurityAuth"/>
		<rdfs:comment xml:lang="en">Java API part implementing the javax.security.auth.kerberos package for J2SE 1.4</rdfs:comment>
	</owl:Class>
	<owl:Class rdf:about="&j2se-1_4;JavaxSecurityAuthLogin">
		<rdfs:subClassOf rdf:resource="&java;JavaAPIPart"/>
		<rdfs:seeAlso rdf:resource="&j2se-1_4;JavaSecurity"/>
		<rdfs:seeAlso rdf:resource="&j2se-1_4;JavaUtil"/>
		<rdfs:seeAlso rdf:resource="&j2se-1_4;JavaxSecurityAuthCallback"/>
		<rdfs:seeAlso rdf:resource="&j2se-1_4;JavaLang"/>
		<rdfs:seeAlso rdf:resource="&j2se-1_4;JavaxSecurityAuth"/>
		<rdfs:comment xml:lang="en">Java API part implementing the javax.security.auth.login package for J2SE 1.4</rdfs:comment>
	</owl:Class>
	<owl:Class rdf:about="&j2se-1_4;JavaxSecurityAuthSpi">
		<rdfs:subClassOf rdf:resource="&java;JavaAPIPart"/>
		<rdfs:seeAlso rdf:resource="&j2se-1_4;JavaUtil"/>
		<rdfs:seeAlso rdf:resource="&j2se-1_4;JavaxSecurityAuthCallback"/>
		<rdfs:seeAlso rdf:resource="&j2se-1_4;JavaxSecurityAuth"/>
		<rdfs:comment xml:lang="en">Java API part implementing the javax.security.auth.spi package for J2SE 1.4</rdfs:comment>
	</owl:Class>
	<owl:Class rdf:about="&j2se-1_4;JavaxSecurityCert">
		<rdfs:subClassOf rdf:resource="&java;JavaAPIPart"/>
		<rdfs:seeAlso rdf:resource="&j2se-1_4;JavaSecurity"/>
		<rdfs:seeAlso rdf:resource="&j2se-1_4;JavaUtil"/>
		<rdfs:seeAlso rdf:resource="&j2se-1_4;JavaLang"/>
		<rdfs:seeAlso rdf:resource="&j2se-1_4;JavaIo"/>
		<rdfs:seeAlso rdf:resource="&j2se-1_4;JavaMath"/>
		<rdfs:comment xml:lang="en">Java API part implementing the javax.security.cert package for J2SE 1.4</rdfs:comment>
	</owl:Class>
	<owl:Class rdf:about="&j2se-1_4;JavaxNaming">
		<rdfs:subClassOf rdf:resource="&j2se-1_3;JavaxNaming"/>
		<rdfs:seeAlso rdf:resource="&j2se-1_4;JavaUtil"/>
		<rdfs:seeAlso rdf:resource="&j2se-1_4;JavaLang"/>
		<rdfs:seeAlso rdf:resource="&j2se-1_4;JavaIo"/>
		<rdfs:comment xml:lang="en">Java API part implementing the javax.naming package for J2SE 1.4</rdfs:comment>
	</owl:Class>
	<owl:Class rdf:about="&j2se-1_4;JavaxNamingDirectory">
		<rdfs:subClassOf rdf:resource="&j2se-1_3;JavaxNamingDirectory"/>
		<rdfs:seeAlso rdf:resource="&j2se-1_4;JavaUtil"/>
		<rdfs:seeAlso rdf:resource="&j2se-1_4;JavaxNaming"/>
		<rdfs:seeAlso rdf:resource="&j2se-1_4;JavaLang"/>
		<rdfs:seeAlso rdf:resource="&j2se-1_4;JavaIo"/>
		<rdfs:comment xml:lang="en">Java API part implementing the javax.naming.directory package for J2SE 1.4</rdfs:comment>
	</owl:Class>
	<owl:Class rdf:about="&j2se-1_4;JavaxNamingEvent">
		<owl:equivalentClass rdf:resource="&j2se-1_3;JavaxNamingEvent"/>
		<rdfs:subClassOf rdf:resource="&java;JavaAPIPart"/>
		<rdfs:seeAlso rdf:resource="&j2se-1_4;JavaUtil"/>
		<rdfs:seeAlso rdf:resource="&j2se-1_4;JavaxNaming"/>
		<rdfs:seeAlso rdf:resource="&j2se-1_4;JavaLang"/>
		<rdfs:seeAlso rdf:resource="&j2se-1_4;JavaxNamingDirectory"/>
		<rdfs:comment xml:lang="en">Java API part implementing the javax.naming.event package for J2SE 1.4</rdfs:comment>
	</owl:Class>
	<owl:Class rdf:about="&j2se-1_4;JavaxNamingLdap">
		<rdfs:subClassOf rdf:resource="&j2se-1_3;JavaxNamingLdap"/>
		<rdfs:seeAlso rdf:resource="&j2se-1_4;JavaxNamingEvent"/>
		<rdfs:seeAlso rdf:resource="&j2se-1_4;JavaxNetSsl"/>
		<rdfs:seeAlso rdf:resource="&j2se-1_4;JavaUtil"/>
		<rdfs:seeAlso rdf:resource="&j2se-1_4;JavaxNaming"/>
		<rdfs:seeAlso rdf:resource="&j2se-1_4;JavaLang"/>
		<rdfs:seeAlso rdf:resource="&j2se-1_4;JavaxNamingDirectory"/>
		<rdfs:seeAlso rdf:resource="&j2se-1_4;JavaIo"/>
		<rdfs:comment xml:lang="en">Java API part implementing the javax.naming.ldap package for J2SE 1.4</rdfs:comment>
	</owl:Class>
	<owl:Class rdf:about="&j2se-1_4;JavaxNamingSpi">
		<owl:equivalentClass rdf:resource="&j2se-1_3;JavaxNamingSpi"/>
		<rdfs:subClassOf rdf:resource="&java;JavaAPIPart"/>
		<rdfs:seeAlso rdf:resource="&j2se-1_4;JavaUtil"/>
		<rdfs:seeAlso rdf:resource="&j2se-1_4;JavaxNaming"/>
		<rdfs:seeAlso rdf:resource="&j2se-1_4;JavaLang"/>
		<rdfs:seeAlso rdf:resource="&j2se-1_4;JavaxNamingDirectory"/>
		<rdfs:seeAlso rdf:resource="&j2se-1_4;JavaIo"/>
		<rdfs:comment xml:lang="en">Java API part implementing the javax.naming.spi package for J2SE 1.4</rdfs:comment>
	</owl:Class>
	<owl:Class rdf:about="&j2se-1_4;JavaxNet">
		<rdfs:subClassOf rdf:resource="&java;JavaAPIPart"/>
		<rdfs:seeAlso rdf:resource="&j2se-1_4;JavaNet"/>
		<rdfs:seeAlso rdf:resource="&j2se-1_4;JavaLang"/>
		<rdfs:comment xml:lang="en">Java API part implementing the javax.net package for J2SE 1.4</rdfs:comment>
	</owl:Class>
	<owl:Class rdf:about="&j2se-1_4;JavaxNetSsl">
		<rdfs:subClassOf rdf:resource="&java;JavaAPIPart"/>
		<rdfs:seeAlso rdf:resource="&j2se-1_4;JavaNet"/>
		<rdfs:seeAlso rdf:resource="&j2se-1_4;JavaUtil"/>
		<rdfs:seeAlso rdf:resource="&j2se-1_4;JavaSecurity"/>
		<rdfs:seeAlso rdf:resource="&j2se-1_4;JavaLang"/>
		<rdfs:seeAlso rdf:resource="&j2se-1_4;JavaIo"/>
		<rdfs:seeAlso rdf:resource="&j2se-1_4;JavaxNet"/>
		<rdfs:comment xml:lang="en">Java API part implementing the javax.net.ssl package for J2SE 1.4</rdfs:comment>
	</owl:Class>
	<owl:Class rdf:about="&j2se-1_4;JavaxRmi">
		<owl:equivalentClass rdf:resource="&j2se-1_3;JavaxRmi"/>
		<rdfs:subClassOf rdf:resource="&java;JavaAPIPart"/>
		<rdfs:seeAlso rdf:resource="&j2se-1_4;JavaLang"/>
		<rdfs:seeAlso rdf:resource="&j2se-1_4;JavaRmi"/>
		<rdfs:comment xml:lang="en">Java API part implementing the javax.rmi package for J2SE 1.4</rdfs:comment>
	</owl:Class>
	<owl:Class rdf:about="&j2se-1_4;JavaxRmiCORBA">
		<owl:equivalentClass rdf:resource="&j2se-1_3;JavaxRmiCORBA"/>
		<rdfs:subClassOf rdf:resource="&java;JavaAPIPart"/>
		<rdfs:seeAlso rdf:resource="&j2se-1_4;OrgOmgCORBA_2_3Portable"/>
		<rdfs:seeAlso rdf:resource="&j2se-1_4;OrgOmgCORBA"/>
		<rdfs:seeAlso rdf:resource="&j2se-1_4;OrgOmgSendingContext"/>
		<rdfs:seeAlso rdf:resource="&j2se-1_4;OrgOmgCORBAPortable"/>
		<rdfs:seeAlso rdf:resource="&j2se-1_4;JavaLang"/>
		<rdfs:seeAlso rdf:resource="&j2se-1_4;JavaIo"/>
		<rdfs:seeAlso rdf:resource="&j2se-1_4;JavaRmi"/>
		<rdfs:comment xml:lang="en">Java API part implementing the javax.rmi.CORBA package for J2SE 1.4</rdfs:comment>
	</owl:Class>
	<owl:Class rdf:about="&j2se-1_4;JavaxCrypto">
		<rdfs:subClassOf rdf:resource="&java;JavaAPIPart"/>
		<rdfs:seeAlso rdf:resource="&j2se-1_4;JavaSecurityCert"/>
		<rdfs:seeAlso rdf:resource="&j2se-1_4;JavaSecurity"/>
		<rdfs:seeAlso rdf:resource="&j2se-1_4;JavaSecuritySpec"/>
		<rdfs:seeAlso rdf:resource="&j2se-1_4;JavaLang"/>
		<rdfs:seeAlso rdf:resource="&j2se-1_4;JavaIo"/>
		<rdfs:comment xml:lang="en">Java API part implementing the javax.crypto package for J2SE 1.4</rdfs:comment>
	</owl:Class>
	<owl:Class rdf:about="&j2se-1_4;JavaxCryptoInterfaces">
		<rdfs:subClassOf rdf:resource="&java;JavaAPIPart"/>
		<rdfs:seeAlso rdf:resource="&j2se-1_4;JavaSecurity"/>
		<rdfs:seeAlso rdf:resource="&j2se-1_4;JavaxCrypto"/>
		<rdfs:seeAlso rdf:resource="&j2se-1_4;JavaxCryptoSpec"/>
		<rdfs:seeAlso rdf:resource="&j2se-1_4;JavaMath"/>
		<rdfs:comment xml:lang="en">Java API part implementing the javax.crypto.interfaces package for J2SE 1.4</rdfs:comment>
	</owl:Class>
	<owl:Class rdf:about="&j2se-1_4;JavaxCryptoSpec">
		<rdfs:subClassOf rdf:resource="&java;JavaAPIPart"/>
		<rdfs:seeAlso rdf:resource="&j2se-1_4;JavaSecuritySpec"/>
		<rdfs:seeAlso rdf:resource="&j2se-1_4;JavaLang"/>
		<rdfs:seeAlso rdf:resource="&j2se-1_4;JavaxCrypto"/>
		<rdfs:seeAlso rdf:resource="&j2se-1_4;JavaMath"/>
		<rdfs:comment xml:lang="en">Java API part implementing the javax.crypto.spec package for J2SE 1.4</rdfs:comment>
	</owl:Class>
	<owl:Class rdf:about="&j2se-1_4;JavaxSql">
		<rdfs:subClassOf rdf:resource="&java;JavaAPIPart"/>
		<rdfs:seeAlso rdf:resource="&j2se-1_4;JavaxTransactionXa"/>
		<rdfs:seeAlso rdf:resource="&j2se-1_4;JavaSql"/>
		<rdfs:seeAlso rdf:resource="&j2se-1_4;JavaMath"/>
		<rdfs:seeAlso rdf:resource="&j2se-1_4;JavaUtil"/>
		<rdfs:seeAlso rdf:resource="&j2se-1_4;JavaLang"/>
		<rdfs:seeAlso rdf:resource="&j2se-1_4;JavaIo"/>
		<rdfs:comment xml:lang="en">Java API part implementing the javax.sql package for J2SE 1.4</rdfs:comment>
	</owl:Class>
	<owl:Class rdf:about="&j2se-1_4;JavaxTransaction">
		<rdfs:subClassOf rdf:resource="&j2se-1_3;JavaxTransaction"/>
		<rdfs:seeAlso rdf:resource="&j2se-1_4;JavaLang"/>
		<rdfs:seeAlso rdf:resource="&j2se-1_4;JavaRmi"/>
		<rdfs:comment xml:lang="en">Java API part implementing the javax.transaction package for J2SE 1.4</rdfs:comment>
	</owl:Class>
	<owl:Class rdf:about="&j2se-1_4;JavaxTransactionXa">
		<rdfs:subClassOf rdf:resource="&java;JavaAPIPart"/>
		<rdfs:seeAlso rdf:resource="&j2se-1_4;JavaLang"/>
		<rdfs:comment xml:lang="en">Java API part implementing the javax.transaction.xa package for J2SE 1.4</rdfs:comment>
	</owl:Class>
	<owl:Class rdf:about="&j2se-1_4;JavaxXmlParsers">
		<rdfs:subClassOf rdf:resource="&java;JavaAPIPart"/>
		<rdfs:seeAlso rdf:resource="&j2se-1_4;OrgXmlSax"/>
		<rdfs:seeAlso rdf:resource="&j2se-1_4;OrgXmlSaxHelpers"/>
		<rdfs:seeAlso rdf:resource="&j2se-1_4;OrgW3cDom"/>
		<rdfs:seeAlso rdf:resource="&j2se-1_4;JavaLang"/>
		<rdfs:seeAlso rdf:resource="&j2se-1_4;JavaIo"/>
		<rdfs:comment xml:lang="en">Java API part implementing the javax.xml.parsers package for J2SE 1.4</rdfs:comment>
	</owl:Class>
	<owl:Class rdf:about="&j2se-1_4;JavaxXmlTransform">
		<rdfs:subClassOf rdf:resource="&java;JavaAPIPart"/>
		<rdfs:seeAlso rdf:resource="&j2se-1_4;JavaUtil"/>
		<rdfs:seeAlso rdf:resource="&j2se-1_4;JavaLang"/>
		<rdfs:seeAlso rdf:resource="&j2se-1_4;JavaIo"/>
		<rdfs:comment xml:lang="en">Java API part implementing the javax.xml.transform package for J2SE 1.4</rdfs:comment>
	</owl:Class>
	<owl:Class rdf:about="&j2se-1_4;JavaxXmlTransformDom">
		<rdfs:subClassOf rdf:resource="&java;JavaAPIPart"/>
		<rdfs:seeAlso rdf:resource="&j2se-1_4;JavaLang"/>
		<rdfs:seeAlso rdf:resource="&j2se-1_4;JavaxXmlTransform"/>
		<rdfs:seeAlso rdf:resource="&j2se-1_4;OrgW3cDom"/>
		<rdfs:comment xml:lang="en">Java API part implementing the javax.xml.transform.dom package for J2SE 1.4</rdfs:comment>
	</owl:Class>
	<owl:Class rdf:about="&j2se-1_4;JavaxXmlTransformSax">
		<rdfs:subClassOf rdf:resource="&java;JavaAPIPart"/>
		<rdfs:seeAlso rdf:resource="&j2se-1_4;OrgXmlSax"/>
		<rdfs:seeAlso rdf:resource="&j2se-1_4;JavaxXmlTransform"/>
		<rdfs:seeAlso rdf:resource="&j2se-1_4;JavaLang"/>
		<rdfs:seeAlso rdf:resource="&j2se-1_4;OrgXmlSaxExt"/>
		<rdfs:comment xml:lang="en">Java API part implementing the javax.xml.transform.sax package for J2SE 1.4</rdfs:comment>
	</owl:Class>
	<owl:Class rdf:about="&j2se-1_4;JavaxXmlTransformStream">
		<rdfs:subClassOf rdf:resource="&java;JavaAPIPart"/>
		<rdfs:seeAlso rdf:resource="&j2se-1_4;JavaLang"/>
		<rdfs:seeAlso rdf:resource="&j2se-1_4;JavaIo"/>
		<rdfs:seeAlso rdf:resource="&j2se-1_4;JavaxXmlTransform"/>
		<rdfs:comment xml:lang="en">Java API part implementing the javax.xml.transform.stream package for J2SE 1.4</rdfs:comment>
	</owl:Class>
	<owl:Class rdf:about="&j2se-1_4;OrgW3cDom">
		<rdfs:subClassOf rdf:resource="&java;JavaAPIPart"/>
		<rdfs:seeAlso rdf:resource="&j2se-1_4;JavaLang"/>
		<rdfs:comment xml:lang="en">Java API part implementing the org.w3c.dom package for J2SE 1.4</rdfs:comment>
	</owl:Class>
	<owl:Class rdf:about="&j2se-1_4;OrgW3cDomCss">
		<rdfs:subClassOf rdf:resource="&java;JavaAPIPart"/>
		<rdfs:seeAlso rdf:resource="&j2se-1_4;JavaLang"/>
		<rdfs:seeAlso rdf:resource="&j2se-1_4;OrgW3cDomViews"/>
		<rdfs:seeAlso rdf:resource="&j2se-1_4;OrgW3cDom"/>
		<rdfs:seeAlso rdf:resource="&j2se-1_4;OrgW3cDomStylesheets"/>
		<rdfs:comment xml:lang="en">Java API part implementing the org.w3c.dom.css package for J2SE 1.4</rdfs:comment>
	</owl:Class>
	<owl:Class rdf:about="&j2se-1_4;OrgW3cDomStylesheets">
		<rdfs:subClassOf rdf:resource="&java;JavaAPIPart"/>
		<rdfs:seeAlso rdf:resource="&j2se-1_4;JavaLang"/>
		<rdfs:seeAlso rdf:resource="&j2se-1_4;OrgW3cDom"/>
		<rdfs:comment xml:lang="en">Java API part implementing the org.w3c.dom.stylesheets package for J2SE 1.4</rdfs:comment>
	</owl:Class>
	<owl:Class rdf:about="&j2se-1_4;OrgW3cDomViews">
		<rdfs:subClassOf rdf:resource="&java;JavaAPIPart"/>
		<rdfs:comment xml:lang="en">Java API part implementing the org.w3c.dom.views package for J2SE 1.4</rdfs:comment>
	</owl:Class>
	<owl:Class rdf:about="&j2se-1_4;OrgW3cDomEvents">
		<rdfs:subClassOf rdf:resource="&java;JavaAPIPart"/>
		<rdfs:seeAlso rdf:resource="&j2se-1_4;JavaLang"/>
		<rdfs:seeAlso rdf:resource="&j2se-1_4;OrgW3cDomViews"/>
		<rdfs:seeAlso rdf:resource="&j2se-1_4;OrgW3cDom"/>
		<rdfs:comment xml:lang="en">Java API part implementing the org.w3c.dom.events package for J2SE 1.4</rdfs:comment>
	</owl:Class>
	<owl:Class rdf:about="&j2se-1_4;OrgW3cDomHtml">
		<rdfs:subClassOf rdf:resource="&java;JavaAPIPart"/>
		<rdfs:seeAlso rdf:resource="&j2se-1_4;JavaLang"/>
		<rdfs:seeAlso rdf:resource="&j2se-1_4;OrgW3cDom"/>
		<rdfs:comment xml:lang="en">Java API part implementing the org.w3c.dom.html package for J2SE 1.4</rdfs:comment>
	</owl:Class>
	<owl:Class rdf:about="&j2se-1_4;OrgW3cDomTraversal">
		<rdfs:subClassOf rdf:resource="&java;JavaAPIPart"/>
		<rdfs:seeAlso rdf:resource="&j2se-1_4;OrgW3cDom"/>
		<rdfs:comment xml:lang="en">Java API part implementing the org.w3c.dom.traversal package for J2SE 1.4</rdfs:comment>
	</owl:Class>
	<owl:Class rdf:about="&j2se-1_4;OrgOmgCORBA_2_3">
		<owl:equivalentClass rdf:resource="&j2se-1_3;OrgOmgCORBA_2_3"/>
		<rdfs:subClassOf rdf:resource="&java;JavaAPIPart"/>
		<rdfs:seeAlso rdf:resource="&j2se-1_4;OrgOmgCORBAPortable"/>
		<rdfs:seeAlso rdf:resource="&j2se-1_4;JavaLang"/>
		<rdfs:seeAlso rdf:resource="&j2se-1_4;OrgOmgCORBA"/>
		<rdfs:comment xml:lang="en">Java API part implementing the org.omg.CORBA_2_3 package for J2SE 1.4</rdfs:comment>
	</owl:Class>
	<owl:Class rdf:about="&j2se-1_4;OrgOmgCORBA_2_3Portable">
		<rdfs:subClassOf rdf:resource="&java;JavaAPIPart"/>
		<rdfs:seeAlso rdf:resource="&j2se-1_4;JavaLang"/>
		<rdfs:seeAlso rdf:resource="&j2se-1_4;OrgOmgCORBAPortable"/>
		<rdfs:seeAlso rdf:resource="&j2se-1_4;OrgOmgCORBA"/>
		<rdfs:seeAlso rdf:resource="&j2se-1_4;JavaIo"/>
		<rdfs:comment xml:lang="en">Java API part implementing the org.omg.CORBA_2_3.portable package for J2SE 1.4</rdfs:comment>
	</owl:Class>
	<owl:Class rdf:about="&j2se-1_4;OrgOmgCORBA">
		<rdfs:subClassOf rdf:resource="&java;JavaAPIPart"/>
		<rdfs:seeAlso rdf:resource="&j2se-1_4;JavaMath"/>
		<rdfs:seeAlso rdf:resource="&j2se-1_4;JavaApplet"/>
		<rdfs:seeAlso rdf:resource="&j2se-1_4;JavaUtil"/>
		<rdfs:seeAlso rdf:resource="&j2se-1_4;JavaLang"/>
		<rdfs:seeAlso rdf:resource="&j2se-1_4;OrgOmgCORBAPortable"/>
		<rdfs:seeAlso rdf:resource="&j2se-1_4;JavaIo"/>
		<rdfs:comment xml:lang="en">Java API part implementing the org.omg.CORBA package for J2SE 1.4</rdfs:comment>
	</owl:Class>
	<owl:Class rdf:about="&j2se-1_4;OrgOmgCORBAPortable">
		<rdfs:subClassOf rdf:resource="&java;JavaAPIPart"/>
		<rdfs:seeAlso rdf:resource="&j2se-1_4;OrgOmgCORBA"/>
		<rdfs:seeAlso rdf:resource="&j2se-1_4;JavaMath"/>
		<rdfs:seeAlso rdf:resource="&j2se-1_4;JavaLang"/>
		<rdfs:seeAlso rdf:resource="&j2se-1_4;JavaIo"/>
		<rdfs:seeAlso rdf:resource="&j2se-1_4;OrgOmgCORBA_2_3Portable"/>
		<rdfs:comment xml:lang="en">Java API part implementing the org.omg.CORBA.portable package for J2SE 1.4</rdfs:comment>
	</owl:Class>
	<owl:Class rdf:about="&j2se-1_4;OrgOmgCORBADynAnyPackage">
		<rdfs:subClassOf rdf:resource="&j2se-1_3;OrgOmgCORBADynAnyPackage"/>
		<rdfs:seeAlso rdf:resource="&j2se-1_4;JavaLang"/>
		<rdfs:seeAlso rdf:resource="&j2se-1_4;OrgOmgCORBA"/>
		<rdfs:comment xml:lang="en">Java API part implementing the org.omg.CORBA.DynAnyPackage package for J2SE 1.4</rdfs:comment>
	</owl:Class>
	<owl:Class rdf:about="&j2se-1_4;OrgOmgCORBAORBPackage">
		<rdfs:subClassOf rdf:resource="&j2se-1_3;OrgOmgCORBAORBPackage"/>
		<rdfs:seeAlso rdf:resource="&j2se-1_4;JavaLang"/>
		<rdfs:seeAlso rdf:resource="&j2se-1_4;OrgOmgCORBA"/>
		<rdfs:comment xml:lang="en">Java API part implementing the org.omg.CORBA.ORBPackage package for J2SE 1.4</rdfs:comment>
	</owl:Class>
	<owl:Class rdf:about="&j2se-1_4;OrgOmgCORBATypeCodePackage">
		<rdfs:subClassOf rdf:resource="&j2se-1_3;OrgOmgCORBATypeCodePackage"/>
		<rdfs:seeAlso rdf:resource="&j2se-1_4;JavaLang"/>
		<rdfs:seeAlso rdf:resource="&j2se-1_4;OrgOmgCORBA"/>
		<rdfs:comment xml:lang="en">Java API part implementing the org.omg.CORBA.TypeCodePackage package for J2SE 1.4</rdfs:comment>
	</owl:Class>
	<owl:Class rdf:about="&j2se-1_4;OrgOmgSendingContext">
		<owl:equivalentClass rdf:resource="&j2se-1_3;OrgOmgSendingContext"/>
		<rdfs:subClassOf rdf:resource="&java;JavaAPIPart"/>
		<rdfs:seeAlso rdf:resource="&j2se-1_4;OrgOmgCORBAPortable"/>
		<rdfs:seeAlso rdf:resource="&j2se-1_4;OrgOmgCORBA"/>
		<rdfs:comment xml:lang="en">Java API part implementing the org.omg.SendingContext package for J2SE 1.4</rdfs:comment>
	</owl:Class>
	<owl:Class rdf:about="&j2se-1_4;OrgOmgCosNaming">
		<rdfs:subClassOf rdf:resource="&java;JavaAPIPart"/>
		<rdfs:seeAlso rdf:resource="&j2se-1_4;OrgOmgCORBA"/>
		<rdfs:seeAlso rdf:resource="&j2se-1_4;OrgOmgPortableServer"/>
		<rdfs:seeAlso rdf:resource="&j2se-1_4;JavaLang"/>
		<rdfs:seeAlso rdf:resource="&j2se-1_4;OrgOmgCORBAPortable"/>
		<rdfs:comment xml:lang="en">Java API part implementing the org.omg.CosNaming package for J2SE 1.4</rdfs:comment>
	</owl:Class>
	<owl:Class rdf:about="&j2se-1_4;OrgOmgCosNamingNamingContextExtPackage">
		<rdfs:subClassOf rdf:resource="&java;JavaAPIPart"/>
		<rdfs:seeAlso rdf:resource="&j2se-1_4;OrgOmgCORBAPortable"/>
		<rdfs:seeAlso rdf:resource="&j2se-1_4;JavaLang"/>
		<rdfs:seeAlso rdf:resource="&j2se-1_4;OrgOmgCORBA"/>
		<rdfs:comment xml:lang="en">Java API part implementing the org.omg.CosNaming.NamingContextExtPackage package for J2SE 1.4</rdfs:comment>
	</owl:Class>
	<owl:Class rdf:about="&j2se-1_4;OrgOmgCosNamingNamingContextPackage">
		<rdfs:subClassOf rdf:resource="&java;JavaAPIPart"/>
		<rdfs:seeAlso rdf:resource="&j2se-1_4;OrgOmgCORBAPortable"/>
		<rdfs:seeAlso rdf:resource="&j2se-1_4;JavaLang"/>
		<rdfs:seeAlso rdf:resource="&j2se-1_4;OrgOmgCORBA"/>
		<rdfs:seeAlso rdf:resource="&j2se-1_4;OrgOmgCosNaming"/>
		<rdfs:comment xml:lang="en">Java API part implementing the org.omg.CosNaming.NamingContextPackage package for J2SE 1.4</rdfs:comment>
	</owl:Class>
	<owl:Class rdf:about="&j2se-1_4;OrgOmgPortableServer">
		<rdfs:subClassOf rdf:resource="&java;JavaAPIPart"/>
		<rdfs:seeAlso rdf:resource="&j2se-1_4;OrgOmgPortableServerPOAManagerPackage"/>
		<rdfs:seeAlso rdf:resource="&j2se-1_4;OrgOmgPortableServerPortable"/>
		<rdfs:seeAlso rdf:resource="&j2se-1_4;OrgOmgCORBA"/>
		<rdfs:seeAlso rdf:resource="&j2se-1_4;JavaLang"/>
		<rdfs:seeAlso rdf:resource="&j2se-1_4;OrgOmgCORBAPortable"/>
		<rdfs:seeAlso rdf:resource="&j2se-1_4;OrgOmgPortableServerServantLocatorPackage"/>
		<rdfs:comment xml:lang="en">Java API part implementing the org.omg.PortableServer package for J2SE 1.4</rdfs:comment>
	</owl:Class>
	<owl:Class rdf:about="&j2se-1_4;OrgOmgPortableServerCurrentPackage">
		<rdfs:subClassOf rdf:resource="&java;JavaAPIPart"/>
		<rdfs:seeAlso rdf:resource="&j2se-1_4;OrgOmgCORBAPortable"/>
		<rdfs:seeAlso rdf:resource="&j2se-1_4;JavaLang"/>
		<rdfs:seeAlso rdf:resource="&j2se-1_4;OrgOmgCORBA"/>
		<rdfs:comment xml:lang="en">Java API part implementing the org.omg.PortableServer.CurrentPackage package for J2SE 1.4</rdfs:comment>
	</owl:Class>
	<owl:Class rdf:about="&j2se-1_4;OrgOmgPortableServerPOAManagerPackage">
		<rdfs:subClassOf rdf:resource="&java;JavaAPIPart"/>
		<rdfs:seeAlso rdf:resource="&j2se-1_4;JavaLang"/>
		<rdfs:seeAlso rdf:resource="&j2se-1_4;OrgOmgCORBAPortable"/>
		<rdfs:seeAlso rdf:resource="&j2se-1_4;OrgOmgCORBA"/>
		<rdfs:comment xml:lang="en">Java API part implementing the org.omg.PortableServer.POAManagerPackage package for J2SE 1.4</rdfs:comment>
	</owl:Class>
	<owl:Class rdf:about="&j2se-1_4;OrgOmgPortableServerPOAPackage">
		<rdfs:subClassOf rdf:resource="&java;JavaAPIPart"/>
		<rdfs:seeAlso rdf:resource="&j2se-1_4;OrgOmgCORBAPortable"/>
		<rdfs:seeAlso rdf:resource="&j2se-1_4;JavaLang"/>
		<rdfs:seeAlso rdf:resource="&j2se-1_4;OrgOmgCORBA"/>
		<rdfs:comment xml:lang="en">Java API part implementing the org.omg.PortableServer.POAPackage package for J2SE 1.4</rdfs:comment>
	</owl:Class>
	<owl:Class rdf:about="&j2se-1_4;OrgOmgPortableServerPortable">
		<rdfs:subClassOf rdf:resource="&java;JavaAPIPart"/>
		<rdfs:seeAlso rdf:resource="&j2se-1_4;JavaLang"/>
		<rdfs:seeAlso rdf:resource="&j2se-1_4;OrgOmgCORBA"/>
		<rdfs:seeAlso rdf:resource="&j2se-1_4;OrgOmgPortableServer"/>
		<rdfs:comment xml:lang="en">Java API part implementing the org.omg.PortableServer.portable package for J2SE 1.4</rdfs:comment>
	</owl:Class>
	<owl:Class rdf:about="&j2se-1_4;OrgOmgPortableServerServantLocatorPackage">
		<rdfs:subClassOf rdf:resource="&java;JavaAPIPart"/>
		<rdfs:seeAlso rdf:resource="&j2se-1_4;OrgOmgCORBAPortable"/>
		<rdfs:seeAlso rdf:resource="&j2se-1_4;JavaLang"/>
		<rdfs:seeAlso rdf:resource="&j2se-1_4;OrgOmgCORBA"/>
		<rdfs:comment xml:lang="en">Java API part implementing the org.omg.PortableServer.ServantLocatorPackage package for J2SE 1.4</rdfs:comment>
	</owl:Class>
	<owl:Class rdf:about="&j2se-1_4;OrgOmgDynamic">
		<rdfs:subClassOf rdf:resource="&java;JavaAPIPart"/>
		<rdfs:seeAlso rdf:resource="&j2se-1_4;JavaLang"/>
		<rdfs:seeAlso rdf:resource="&j2se-1_4;OrgOmgCORBAPortable"/>
		<rdfs:seeAlso rdf:resource="&j2se-1_4;OrgOmgCORBA"/>
		<rdfs:comment xml:lang="en">Java API part implementing the org.omg.Dynamic package for J2SE 1.4</rdfs:comment>
	</owl:Class>
	<owl:Class rdf:about="&j2se-1_4;OrgOmgDynamicAny">
		<rdfs:subClassOf rdf:resource="&java;JavaAPIPart"/>
		<rdfs:seeAlso rdf:resource="&j2se-1_4;OrgOmgCORBA"/>
		<rdfs:seeAlso rdf:resource="&j2se-1_4;OrgOmgCORBAPortable"/>
		<rdfs:seeAlso rdf:resource="&j2se-1_4;JavaLang"/>
		<rdfs:seeAlso rdf:resource="&j2se-1_4;JavaIo"/>
		<rdfs:comment xml:lang="en">Java API part implementing the org.omg.DynamicAny package for J2SE 1.4</rdfs:comment>
	</owl:Class>
	<owl:Class rdf:about="&j2se-1_4;OrgOmgDynamicAnyDynAnyFactoryPackage">
		<rdfs:subClassOf rdf:resource="&java;JavaAPIPart"/>
		<rdfs:seeAlso rdf:resource="&j2se-1_4;OrgOmgCORBAPortable"/>
		<rdfs:seeAlso rdf:resource="&j2se-1_4;JavaLang"/>
		<rdfs:seeAlso rdf:resource="&j2se-1_4;OrgOmgCORBA"/>
		<rdfs:comment xml:lang="en">Java API part implementing the org.omg.DynamicAny.DynAnyFactoryPackage package for J2SE 1.4</rdfs:comment>
	</owl:Class>
	<owl:Class rdf:about="&j2se-1_4;OrgOmgDynamicAnyDynAnyPackage">
		<rdfs:subClassOf rdf:resource="&java;JavaAPIPart"/>
		<rdfs:seeAlso rdf:resource="&j2se-1_4;JavaLang"/>
		<rdfs:seeAlso rdf:resource="&j2se-1_4;OrgOmgCORBAPortable"/>
		<rdfs:seeAlso rdf:resource="&j2se-1_4;OrgOmgCORBA"/>
		<rdfs:comment xml:lang="en">Java API part implementing the org.omg.DynamicAny.DynAnyPackage package for J2SE 1.4</rdfs:comment>
	</owl:Class>
	<owl:Class rdf:about="&j2se-1_4;OrgOmgIOP">
		<rdfs:subClassOf rdf:resource="&java;JavaAPIPart"/>
		<rdfs:seeAlso rdf:resource="&j2se-1_4;OrgOmgCORBAPortable"/>
		<rdfs:seeAlso rdf:resource="&j2se-1_4;JavaLang"/>
		<rdfs:seeAlso rdf:resource="&j2se-1_4;OrgOmgCORBA"/>
		<rdfs:comment xml:lang="en">Java API part implementing the org.omg.IOP package for J2SE 1.4</rdfs:comment>
	</owl:Class>
	<owl:Class rdf:about="&j2se-1_4;OrgOmgIOPCodecFactoryPackage">
		<rdfs:subClassOf rdf:resource="&java;JavaAPIPart"/>
		<rdfs:seeAlso rdf:resource="&j2se-1_4;OrgOmgCORBAPortable"/>
		<rdfs:seeAlso rdf:resource="&j2se-1_4;JavaLang"/>
		<rdfs:seeAlso rdf:resource="&j2se-1_4;OrgOmgCORBA"/>
		<rdfs:comment xml:lang="en">Java API part implementing the org.omg.IOP.CodecFactoryPackage package for J2SE 1.4</rdfs:comment>
	</owl:Class>
	<owl:Class rdf:about="&j2se-1_4;OrgOmgIOPCodecPackage">
		<rdfs:subClassOf rdf:resource="&java;JavaAPIPart"/>
		<rdfs:seeAlso rdf:resource="&j2se-1_4;OrgOmgCORBAPortable"/>
		<rdfs:seeAlso rdf:resource="&j2se-1_4;JavaLang"/>
		<rdfs:seeAlso rdf:resource="&j2se-1_4;OrgOmgCORBA"/>
		<rdfs:comment xml:lang="en">Java API part implementing the org.omg.IOP.CodecPackage package for J2SE 1.4</rdfs:comment>
	</owl:Class>
	<owl:Class rdf:about="&j2se-1_4;OrgOmgMessaging">
		<rdfs:subClassOf rdf:resource="&java;JavaAPIPart"/>
		<rdfs:seeAlso rdf:resource="&j2se-1_4;OrgOmgCORBAPortable"/>
		<rdfs:seeAlso rdf:resource="&j2se-1_4;JavaLang"/>
		<rdfs:seeAlso rdf:resource="&j2se-1_4;OrgOmgCORBA"/>
		<rdfs:comment xml:lang="en">Java API part implementing the org.omg.Messaging package for J2SE 1.4</rdfs:comment>
	</owl:Class>
	<owl:Class rdf:about="&j2se-1_4;OrgOmgPortableInterceptor">
		<rdfs:subClassOf rdf:resource="&java;JavaAPIPart"/>
		<rdfs:seeAlso rdf:resource="&j2se-1_4;OrgOmgCORBA"/>
		<rdfs:seeAlso rdf:resource="&j2se-1_4;OrgOmgIOP"/>
		<rdfs:seeAlso rdf:resource="&j2se-1_4;OrgOmgCORBAPortable"/>
		<rdfs:seeAlso rdf:resource="&j2se-1_4;JavaLang"/>
		<rdfs:comment xml:lang="en">Java API part implementing the org.omg.PortableInterceptor package for J2SE 1.4</rdfs:comment>
	</owl:Class>
	<owl:Class rdf:about="&j2se-1_4;OrgOmgPortableInterceptorORBInitInfoPackage">
		<rdfs:subClassOf rdf:resource="&java;JavaAPIPart"/>
		<rdfs:seeAlso rdf:resource="&j2se-1_4;OrgOmgCORBAPortable"/>
		<rdfs:seeAlso rdf:resource="&j2se-1_4;JavaLang"/>
		<rdfs:seeAlso rdf:resource="&j2se-1_4;OrgOmgCORBA"/>
		<rdfs:comment xml:lang="en">Java API part implementing the org.omg.PortableInterceptor.ORBInitInfoPackage package for J2SE 1.4</rdfs:comment>
	</owl:Class>
	<owl:Class rdf:about="&j2se-1_4;OrgOmgStubJavaRmi">
		<owl:equivalentClass rdf:resource="&j2se-1_3;OrgOmgStubJavaRmi"/>
		<rdfs:subClassOf rdf:resource="&java;JavaAPIPart"/>
		<rdfs:seeAlso rdf:resource="&j2se-1_4;JavaRmi"/>
		<rdfs:seeAlso rdf:resource="&j2se-1_4;JavaxRmiCORBA"/>
		<rdfs:comment xml:lang="en">Java API part implementing the org.omg.stub.java.rmi package for J2SE 1.4</rdfs:comment>
	</owl:Class>
	<owl:Class rdf:about="&j2se-1_4;OrgXmlSax">
		<rdfs:subClassOf rdf:resource="&java;JavaAPIPart"/>
		<rdfs:seeAlso rdf:resource="&j2se-1_4;JavaUtil"/>
		<rdfs:seeAlso rdf:resource="&j2se-1_4;JavaLang"/>
		<rdfs:seeAlso rdf:resource="&j2se-1_4;JavaIo"/>
		<rdfs:comment xml:lang="en">Java API part implementing the org.xml.sax package for J2SE 1.4</rdfs:comment>
	</owl:Class>
	<owl:Class rdf:about="&j2se-1_4;OrgXmlSaxHelpers">
		<rdfs:subClassOf rdf:resource="&java;JavaAPIPart"/>
		<rdfs:seeAlso rdf:resource="&j2se-1_4;OrgXmlSax"/>
		<rdfs:seeAlso rdf:resource="&j2se-1_4;JavaUtil"/>
		<rdfs:seeAlso rdf:resource="&j2se-1_4;JavaLang"/>
		<rdfs:comment xml:lang="en">Java API part implementing the org.xml.sax.helpers package for J2SE 1.4</rdfs:comment>
	</owl:Class>
	<owl:Class rdf:about="&j2se-1_4;OrgXmlSaxExt">
		<rdfs:subClassOf rdf:resource="&java;JavaAPIPart"/>
		<rdfs:seeAlso rdf:resource="&j2se-1_4;JavaLang"/>
		<rdfs:comment xml:lang="en">Java API part implementing the org.xml.sax.ext package for J2SE 1.4</rdfs:comment>
	</owl:Class>
	<owl:Class rdf:about="&j2se-1_4;OrgIetfJgss">
		<rdfs:subClassOf rdf:resource="&java;JavaAPIPart"/>
		<rdfs:seeAlso rdf:resource="&j2se-1_4;JavaNet"/>
		<rdfs:seeAlso rdf:resource="&j2se-1_4;JavaSecurity"/>
		<rdfs:seeAlso rdf:resource="&j2se-1_4;JavaLang"/>
		<rdfs:seeAlso rdf:resource="&j2se-1_4;JavaIo"/>
		<rdfs:comment xml:lang="en">Java API part implementing the org.ietf.jgss package for J2SE 1.4</rdfs:comment>
	</owl:Class>
	<owl:Class rdf:about="&j2se-1_4;JavaLangAPI">
		<rdfs:subClassOf rdf:resource="&j2me-pp-1_1;JavaLangAPI"/>
		<rdfs:subClassOf rdf:resource="&j2se-1_3;JavaLangAPI"/>
		<rdfs:comment xml:lang="en">JavaLibrary implementing the java.lang package for J2SE 1.4</rdfs:comment>
		<rdfs:comment xml:lang="OWLManchester">platform:comprisesInterfacePart some JavaLang</rdfs:comment>
	</owl:Class>
	<owl:Class rdf:about="&j2se-1_4;JavaLangReflectAPI">
		<owl:equivalentClass rdf:resource="&j2me-pp-1_1;JavaLangReflectAPI"/>
		<rdfs:subClassOf rdf:resource="&j2se-1_3;JavaLangReflectAPI"/>
		<rdfs:comment xml:lang="en">JavaLibrary implementing the java.lang.reflect package for J2SE 1.4</rdfs:comment>
		<rdfs:comment xml:lang="OWLManchester">platform:comprisesInterfacePart some JavaLangReflect</rdfs:comment>
	</owl:Class>
	<owl:Class rdf:about="&j2se-1_4;JavaLangRefAPI">
		<owl:equivalentClass rdf:resource="&j2me-pp-1_1;JavaLangRefAPI"/>
		<owl:equivalentClass rdf:resource="&j2se-1_3;JavaLangRefAPI"/>
		<rdfs:subClassOf rdf:resource="&java;JavaAPI"/>
		<rdfs:comment xml:lang="en">JavaLibrary implementing the java.lang.ref package for J2SE 1.4</rdfs:comment>
		<rdfs:comment xml:lang="OWLManchester">platform:comprisesInterfacePart some JavaLangRef</rdfs:comment>
	</owl:Class>
	<owl:Class rdf:about="&j2se-1_4;JavaIoAPI">
		<rdfs:subClassOf rdf:resource="&j2me-pp-1_1;JavaIoAPI"/>
		<rdfs:subClassOf rdf:resource="&j2se-1_3;JavaIoAPI"/>
		<rdfs:comment xml:lang="en">JavaLibrary implementing the java.io package for J2SE 1.4</rdfs:comment>
		<rdfs:comment xml:lang="OWLManchester">platform:comprisesInterfacePart some JavaIo</rdfs:comment>
	</owl:Class>
	<owl:Class rdf:about="&j2se-1_4;JavaUtilAPI">
		<rdfs:subClassOf rdf:resource="&j2me-pp-1_1;JavaUtilAPI"/>
		<rdfs:subClassOf rdf:resource="&j2se-1_3;JavaUtilAPI"/>
		<rdfs:comment xml:lang="en">JavaLibrary implementing the java.util package for J2SE 1.4</rdfs:comment>
		<rdfs:comment xml:lang="OWLManchester">platform:comprisesInterfacePart some JavaUtil</rdfs:comment>
	</owl:Class>
	<owl:Class rdf:about="&j2se-1_4;JavaUtilLoggingAPI">
		<rdfs:subClassOf rdf:resource="&java;JavaAPI"/>
		<rdfs:comment xml:lang="en">JavaLibrary implementing the java.util.logging package for J2SE 1.4</rdfs:comment>
		<rdfs:comment xml:lang="OWLManchester">platform:comprisesInterfacePart some JavaUtilLogging</rdfs:comment>
	</owl:Class>
	<owl:Class rdf:about="&j2se-1_4;JavaUtilJarAPI">
		<owl:equivalentClass rdf:resource="&j2me-pp-1_1;JavaUtilJarAPI"/>
		<rdfs:subClassOf rdf:resource="&j2se-1_3;JavaUtilJarAPI"/>
		<rdfs:comment xml:lang="en">JavaLibrary implementing the java.util.jar package for J2SE 1.4</rdfs:comment>
		<rdfs:comment xml:lang="OWLManchester">platform:comprisesInterfacePart some JavaUtilJar</rdfs:comment>
	</owl:Class>
	<owl:Class rdf:about="&j2se-1_4;JavaUtilZipAPI">
		<owl:equivalentClass rdf:resource="&j2me-pp-1_1;JavaUtilZipAPI"/>
		<rdfs:subClassOf rdf:resource="&j2se-1_3;JavaUtilZipAPI"/>
		<rdfs:comment xml:lang="en">JavaLibrary implementing the java.util.zip package for J2SE 1.4</rdfs:comment>
		<rdfs:comment xml:lang="OWLManchester">platform:comprisesInterfacePart some JavaUtilZip</rdfs:comment>
	</owl:Class>
	<owl:Class rdf:about="&j2se-1_4;JavaUtilPrefsAPI">
		<rdfs:subClassOf rdf:resource="&java;JavaAPI"/>
		<rdfs:comment xml:lang="en">JavaLibrary implementing the java.util.prefs package for J2SE 1.4</rdfs:comment>
		<rdfs:comment xml:lang="OWLManchester">platform:comprisesInterfacePart some JavaUtilPrefs</rdfs:comment>
	</owl:Class>
	<owl:Class rdf:about="&j2se-1_4;JavaUtilRegexAPI">
		<rdfs:subClassOf rdf:resource="&java;JavaAPI"/>
		<rdfs:comment xml:lang="en">JavaLibrary implementing the java.util.regex package for J2SE 1.4</rdfs:comment>
		<rdfs:comment xml:lang="OWLManchester">platform:comprisesInterfacePart some JavaUtilRegex</rdfs:comment>
	</owl:Class>
	<owl:Class rdf:about="&j2se-1_4;JavaNetAPI">
		<rdfs:subClassOf rdf:resource="&j2me-pp-1_1;JavaNetAPI"/>
		<rdfs:subClassOf rdf:resource="&j2se-1_3;JavaNetAPI"/>
		<rdfs:comment xml:lang="en">JavaLibrary implementing the java.net package for J2SE 1.4</rdfs:comment>
		<rdfs:comment xml:lang="OWLManchester">platform:comprisesInterfacePart some JavaNet</rdfs:comment>
	</owl:Class>
	<owl:Class rdf:about="&j2se-1_4;JavaSecurityAPI">
		<rdfs:subClassOf rdf:resource="&j2me-pp-1_1;JavaSecurityAPI"/>
		<rdfs:subClassOf rdf:resource="&j2se-1_3;JavaSecurityAPI"/>
		<rdfs:comment xml:lang="en">JavaLibrary implementing the java.security package for J2SE 1.4</rdfs:comment>
		<rdfs:comment xml:lang="OWLManchester">platform:comprisesInterfacePart some JavaSecurity</rdfs:comment>
	</owl:Class>
	<owl:Class rdf:about="&j2se-1_4;JavaSecurityCertAPI">
		<rdfs:subClassOf rdf:resource="&j2me-pp-1_1;JavaSecurityCertAPI"/>
		<rdfs:subClassOf rdf:resource="&j2se-1_3;JavaSecurityCertAPI"/>
		<rdfs:comment xml:lang="en">JavaLibrary implementing the java.security.cert package for J2SE 1.4</rdfs:comment>
		<rdfs:comment xml:lang="OWLManchester">platform:comprisesInterfacePart some JavaSecurityCert</rdfs:comment>
	</owl:Class>
	<owl:Class rdf:about="&j2se-1_4;JavaSecuritySpecAPI">
		<rdfs:subClassOf rdf:resource="&j2me-pp-1_1;JavaSecuritySpecAPI"/>
		<rdfs:subClassOf rdf:resource="&j2se-1_3;JavaSecuritySpecAPI"/>
		<rdfs:comment xml:lang="en">JavaLibrary implementing the java.security.spec package for J2SE 1.4</rdfs:comment>
		<rdfs:comment xml:lang="OWLManchester">platform:comprisesInterfacePart some JavaSecuritySpec</rdfs:comment>
	</owl:Class>
	<owl:Class rdf:about="&j2se-1_4;JavaSecurityAclAPI">
		<owl:equivalentClass rdf:resource="&j2me-pp-1_1;JavaSecurityAclAPI"/>
		<rdfs:subClassOf rdf:resource="&j2se-1_3;JavaSecurityAclAPI"/>
		<rdfs:comment xml:lang="en">JavaLibrary implementing the java.security.acl package for J2SE 1.4</rdfs:comment>
		<rdfs:comment xml:lang="OWLManchester">platform:comprisesInterfacePart some JavaSecurityAcl</rdfs:comment>
	</owl:Class>
	<owl:Class rdf:about="&j2se-1_4;JavaSecurityInterfacesAPI">
		<rdfs:subClassOf rdf:resource="&j2me-pp-1_1;JavaSecurityInterfacesAPI"/>
		<rdfs:subClassOf rdf:resource="&j2se-1_3;JavaSecurityInterfacesAPI"/>
		<rdfs:comment xml:lang="en">JavaLibrary implementing the java.security.interfaces package for J2SE 1.4</rdfs:comment>
		<rdfs:comment xml:lang="OWLManchester">platform:comprisesInterfacePart some JavaSecurityInterfaces</rdfs:comment>
	</owl:Class>
	<owl:Class rdf:about="&j2se-1_4;JavaNioAPI">
		<rdfs:subClassOf rdf:resource="&java;JavaAPI"/>
		<rdfs:comment xml:lang="en">JavaLibrary implementing the java.nio package for J2SE 1.4</rdfs:comment>
		<rdfs:comment xml:lang="OWLManchester">platform:comprisesInterfacePart some JavaNio</rdfs:comment>
	</owl:Class>
	<owl:Class rdf:about="&j2se-1_4;JavaNioChannelsAPI">
		<rdfs:subClassOf rdf:resource="&java;JavaAPI"/>
		<rdfs:comment xml:lang="en">JavaLibrary implementing the java.nio.channels package for J2SE 1.4</rdfs:comment>
		<rdfs:comment xml:lang="OWLManchester">platform:comprisesInterfacePart some JavaNioChannels</rdfs:comment>
	</owl:Class>
	<owl:Class rdf:about="&j2se-1_4;JavaNioChannelsSpiAPI">
		<rdfs:subClassOf rdf:resource="&java;JavaAPI"/>
		<rdfs:comment xml:lang="en">JavaLibrary implementing the java.nio.channels.spi package for J2SE 1.4</rdfs:comment>
		<rdfs:comment xml:lang="OWLManchester">platform:comprisesInterfacePart some JavaNioChannelsSpi</rdfs:comment>
	</owl:Class>
	<owl:Class rdf:about="&j2se-1_4;JavaNioCharsetAPI">
		<rdfs:subClassOf rdf:resource="&java;JavaAPI"/>
		<rdfs:comment xml:lang="en">JavaLibrary implementing the java.nio.charset package for J2SE 1.4</rdfs:comment>
		<rdfs:comment xml:lang="OWLManchester">platform:comprisesInterfacePart some JavaNioCharset</rdfs:comment>
	</owl:Class>
	<owl:Class rdf:about="&j2se-1_4;JavaNioCharsetSpiAPI">
		<rdfs:subClassOf rdf:resource="&java;JavaAPI"/>
		<rdfs:comment xml:lang="en">JavaLibrary implementing the java.nio.charset.spi package for J2SE 1.4</rdfs:comment>
		<rdfs:comment xml:lang="OWLManchester">platform:comprisesInterfacePart some JavaNioCharsetSpi</rdfs:comment>
	</owl:Class>
	<owl:Class rdf:about="&j2se-1_4;JavaBeansAPI">
		<rdfs:subClassOf rdf:resource="&j2me-pp-1_1;JavaBeansAPI"/>
		<rdfs:subClassOf rdf:resource="&j2se-1_3;JavaBeansAPI"/>
		<rdfs:comment xml:lang="en">JavaLibrary implementing the java.beans package for J2SE 1.4</rdfs:comment>
		<rdfs:comment xml:lang="OWLManchester">platform:comprisesInterfacePart some JavaBeans</rdfs:comment>
	</owl:Class>
	<owl:Class rdf:about="&j2se-1_4;JavaBeansBeancontextAPI">
		<owl:equivalentClass rdf:resource="&j2se-1_3;JavaBeansBeancontextAPI"/>
		<rdfs:subClassOf rdf:resource="&java;JavaAPI"/>
		<rdfs:comment xml:lang="en">JavaLibrary implementing the java.beans.beancontext package for J2SE 1.4</rdfs:comment>
		<rdfs:comment xml:lang="OWLManchester">platform:comprisesInterfacePart some JavaBeansBeancontext</rdfs:comment>
	</owl:Class>
	<owl:Class rdf:about="&j2se-1_4;JavaAwtAPI">
		<rdfs:subClassOf rdf:resource="&j2me-pp-1_1;JavaAwtAPI"/>
		<rdfs:subClassOf rdf:resource="&j2se-1_3;JavaAwtAPI"/>
		<rdfs:comment xml:lang="en">JavaLibrary implementing the java.awt package for J2SE 1.4</rdfs:comment>
		<rdfs:comment xml:lang="OWLManchester">platform:comprisesInterfacePart some JavaAwt</rdfs:comment>
	</owl:Class>
	<owl:Class rdf:about="&j2se-1_4;JavaAwtImageAPI">
		<rdfs:subClassOf rdf:resource="&j2me-pp-1_1;JavaAwtImageAPI"/>
		<rdfs:subClassOf rdf:resource="&j2se-1_3;JavaAwtImageAPI"/>
		<rdfs:comment xml:lang="en">JavaLibrary implementing the java.awt.image package for J2SE 1.4</rdfs:comment>
		<rdfs:comment xml:lang="OWLManchester">platform:comprisesInterfacePart some JavaAwtImage</rdfs:comment>
	</owl:Class>
	<owl:Class rdf:about="&j2se-1_4;JavaAwtImageRenderableAPI">
		<owl:equivalentClass rdf:resource="&j2se-1_3;JavaAwtImageRenderableAPI"/>
		<rdfs:subClassOf rdf:resource="&java;JavaAPI"/>
		<rdfs:comment xml:lang="en">JavaLibrary implementing the java.awt.image.renderable package for J2SE 1.4</rdfs:comment>
		<rdfs:comment xml:lang="OWLManchester">platform:comprisesInterfacePart some JavaAwtImageRenderable</rdfs:comment>
	</owl:Class>
	<owl:Class rdf:about="&j2se-1_4;JavaAwtDatatransferAPI">
		<rdfs:subClassOf rdf:resource="&j2me-pp-1_1;JavaAwtDatatransferAPI"/>
		<rdfs:subClassOf rdf:resource="&j2se-1_3;JavaAwtDatatransferAPI"/>
		<rdfs:comment xml:lang="en">JavaLibrary implementing the java.awt.datatransfer package for J2SE 1.4</rdfs:comment>
		<rdfs:comment xml:lang="OWLManchester">platform:comprisesInterfacePart some JavaAwtDatatransfer</rdfs:comment>
	</owl:Class>
	<owl:Class rdf:about="&j2se-1_4;JavaAwtDndAPI">
		<rdfs:subClassOf rdf:resource="&j2se-1_3;JavaAwtDndAPI"/>
		<rdfs:comment xml:lang="en">JavaLibrary implementing the java.awt.dnd package for J2SE 1.4</rdfs:comment>
		<rdfs:comment xml:lang="OWLManchester">platform:comprisesInterfacePart some JavaAwtDnd</rdfs:comment>
	</owl:Class>
	<owl:Class rdf:about="&j2se-1_4;JavaAwtEventAPI">
		<rdfs:subClassOf rdf:resource="&j2me-pp-1_1;JavaAwtEventAPI"/>
		<rdfs:subClassOf rdf:resource="&j2se-1_3;JavaAwtEventAPI"/>
		<rdfs:comment xml:lang="en">JavaLibrary implementing the java.awt.event package for J2SE 1.4</rdfs:comment>
		<rdfs:comment xml:lang="OWLManchester">platform:comprisesInterfacePart some JavaAwtEvent</rdfs:comment>
	</owl:Class>
	<owl:Class rdf:about="&j2se-1_4;JavaAwtImAPI">
		<owl:equivalentClass rdf:resource="&j2se-1_3;JavaAwtImAPI"/>
		<rdfs:subClassOf rdf:resource="&j2me-pp-1_1;JavaAwtImAPI"/>
		<rdfs:comment xml:lang="en">JavaLibrary implementing the java.awt.im package for J2SE 1.4</rdfs:comment>
		<rdfs:comment xml:lang="OWLManchester">platform:comprisesInterfacePart some JavaAwtIm</rdfs:comment>
	</owl:Class>
	<owl:Class rdf:about="&j2se-1_4;JavaAwtImSpiAPI">
		<rdfs:subClassOf rdf:resource="&j2se-1_3;JavaAwtImSpiAPI"/>
		<rdfs:comment xml:lang="en">JavaLibrary implementing the java.awt.im.spi package for J2SE 1.4</rdfs:comment>
		<rdfs:comment xml:lang="OWLManchester">platform:comprisesInterfacePart some JavaAwtImSpi</rdfs:comment>
	</owl:Class>
	<owl:Class rdf:about="&j2se-1_4;JavaAwtFontAPI">
		<rdfs:subClassOf rdf:resource="&j2me-pp-1_1;JavaAwtFontAPI"/>
		<rdfs:subClassOf rdf:resource="&j2se-1_3;JavaAwtFontAPI"/>
		<rdfs:comment xml:lang="en">JavaLibrary implementing the java.awt.font package for J2SE 1.4</rdfs:comment>
		<rdfs:comment xml:lang="OWLManchester">platform:comprisesInterfacePart some JavaAwtFont</rdfs:comment>
	</owl:Class>
	<owl:Class rdf:about="&j2se-1_4;JavaAwtGeomAPI">
		<rdfs:subClassOf rdf:resource="&j2se-1_3;JavaAwtGeomAPI"/>
		<rdfs:comment xml:lang="en">JavaLibrary implementing the java.awt.geom package for J2SE 1.4</rdfs:comment>
		<rdfs:comment xml:lang="OWLManchester">platform:comprisesInterfacePart some JavaAwtGeom</rdfs:comment>
	</owl:Class>
	<owl:Class rdf:about="&j2se-1_4;JavaAwtColorAPI">
		<rdfs:subClassOf rdf:resource="&j2me-pp-1_1;JavaAwtColorAPI"/>
		<rdfs:subClassOf rdf:resource="&j2se-1_3;JavaAwtColorAPI"/>
		<rdfs:comment xml:lang="en">JavaLibrary implementing the java.awt.color package for J2SE 1.4</rdfs:comment>
		<rdfs:comment xml:lang="OWLManchester">platform:comprisesInterfacePart some JavaAwtColor</rdfs:comment>
	</owl:Class>
	<owl:Class rdf:about="&j2se-1_4;JavaAwtPrintAPI">
		<rdfs:subClassOf rdf:resource="&j2se-1_3;JavaAwtPrintAPI"/>
		<rdfs:comment xml:lang="en">JavaLibrary implementing the java.awt.print package for J2SE 1.4</rdfs:comment>
		<rdfs:comment xml:lang="OWLManchester">platform:comprisesInterfacePart some JavaAwtPrint</rdfs:comment>
	</owl:Class>
	<owl:Class rdf:about="&j2se-1_4;JavaTextAPI">
		<rdfs:subClassOf rdf:resource="&j2se-1_3;JavaTextAPI"/>
		<rdfs:comment xml:lang="en">JavaLibrary implementing the java.text package for J2SE 1.4</rdfs:comment>
		<rdfs:comment xml:lang="OWLManchester">platform:comprisesInterfacePart some JavaText</rdfs:comment>
	</owl:Class>
	<owl:Class rdf:about="&j2se-1_4;JavaMathAPI">
		<rdfs:subClassOf rdf:resource="&j2me-pp-1_1;JavaMathAPI"/>
		<rdfs:subClassOf rdf:resource="&j2se-1_3;JavaMathAPI"/>
		<rdfs:comment xml:lang="en">JavaLibrary implementing the java.math package for J2SE 1.4</rdfs:comment>
		<rdfs:comment xml:lang="OWLManchester">platform:comprisesInterfacePart some JavaMath</rdfs:comment>
	</owl:Class>
	<owl:Class rdf:about="&j2se-1_4;JavaAppletAPI">
		<rdfs:subClassOf rdf:resource="&j2me-pp-1_1;JavaAppletAPI"/>
		<rdfs:subClassOf rdf:resource="&j2se-1_3;JavaAppletAPI"/>
		<rdfs:comment xml:lang="en">JavaLibrary implementing the java.applet package for J2SE 1.4</rdfs:comment>
		<rdfs:comment xml:lang="OWLManchester">platform:comprisesInterfacePart some JavaApplet</rdfs:comment>
	</owl:Class>
	<owl:Class rdf:about="&j2se-1_4;JavaRmiAPI">
		<rdfs:subClassOf rdf:resource="&j2me-pp-1_1;JavaRmiAPI"/>
		<rdfs:subClassOf rdf:resource="&j2se-1_3;JavaRmiAPI"/>
		<rdfs:comment xml:lang="en">JavaLibrary implementing the java.rmi package for J2SE 1.4</rdfs:comment>
		<rdfs:comment xml:lang="OWLManchester">platform:comprisesInterfacePart some JavaRmi</rdfs:comment>
	</owl:Class>
	<owl:Class rdf:about="&j2se-1_4;JavaRmiActivationAPI">
		<rdfs:subClassOf rdf:resource="&j2se-1_3;JavaRmiActivationAPI"/>
		<rdfs:comment xml:lang="en">JavaLibrary implementing the java.rmi.activation package for J2SE 1.4</rdfs:comment>
		<rdfs:comment xml:lang="OWLManchester">platform:comprisesInterfacePart some JavaRmiActivation</rdfs:comment>
	</owl:Class>
	<owl:Class rdf:about="&j2se-1_4;JavaRmiServerAPI">
		<rdfs:subClassOf rdf:resource="&j2se-1_3;JavaRmiServerAPI"/>
		<rdfs:comment xml:lang="en">JavaLibrary implementing the java.rmi.server package for J2SE 1.4</rdfs:comment>
		<rdfs:comment xml:lang="OWLManchester">platform:comprisesInterfacePart some JavaRmiServer</rdfs:comment>
	</owl:Class>
	<owl:Class rdf:about="&j2se-1_4;JavaRmiDgcAPI">
		<owl:equivalentClass rdf:resource="&j2se-1_3;JavaRmiDgcAPI"/>
		<rdfs:subClassOf rdf:resource="&java;JavaAPI"/>
		<rdfs:comment xml:lang="en">JavaLibrary implementing the java.rmi.dgc package for J2SE 1.4</rdfs:comment>
		<rdfs:comment xml:lang="OWLManchester">platform:comprisesInterfacePart some JavaRmiDgc</rdfs:comment>
	</owl:Class>
	<owl:Class rdf:about="&j2se-1_4;JavaRmiRegistryAPI">
		<owl:equivalentClass rdf:resource="&j2se-1_3;JavaRmiRegistryAPI"/>
		<rdfs:subClassOf rdf:resource="&j2me-pp-1_1;JavaRmiRegistryAPI"/>
		<rdfs:comment xml:lang="en">JavaLibrary implementing the java.rmi.registry package for J2SE 1.4</rdfs:comment>
		<rdfs:comment xml:lang="OWLManchester">platform:comprisesInterfacePart some JavaRmiRegistry</rdfs:comment>
	</owl:Class>
	<owl:Class rdf:about="&j2se-1_4;JavaSqlAPI">
		<rdfs:subClassOf rdf:resource="&j2se-1_3;JavaSqlAPI"/>
		<rdfs:comment xml:lang="en">JavaLibrary implementing the java.sql package for J2SE 1.4</rdfs:comment>
		<rdfs:comment xml:lang="OWLManchester">platform:comprisesInterfacePart some JavaSql</rdfs:comment>
	</owl:Class>
	<owl:Class rdf:about="&j2se-1_4;JavaxImageioAPI">
		<rdfs:subClassOf rdf:resource="&java;JavaAPI"/>
		<rdfs:comment xml:lang="en">JavaLibrary implementing the javax.imageio package for J2SE 1.4</rdfs:comment>
		<rdfs:comment xml:lang="OWLManchester">platform:comprisesInterfacePart some JavaxImageio</rdfs:comment>
	</owl:Class>
	<owl:Class rdf:about="&j2se-1_4;JavaxImageioSpiAPI">
		<rdfs:subClassOf rdf:resource="&java;JavaAPI"/>
		<rdfs:comment xml:lang="en">JavaLibrary implementing the javax.imageio.spi package for J2SE 1.4</rdfs:comment>
		<rdfs:comment xml:lang="OWLManchester">platform:comprisesInterfacePart some JavaxImageioSpi</rdfs:comment>
	</owl:Class>
	<owl:Class rdf:about="&j2se-1_4;JavaxImageioMetadataAPI">
		<rdfs:subClassOf rdf:resource="&java;JavaAPI"/>
		<rdfs:comment xml:lang="en">JavaLibrary implementing the javax.imageio.metadata package for J2SE 1.4</rdfs:comment>
		<rdfs:comment xml:lang="OWLManchester">platform:comprisesInterfacePart some JavaxImageioMetadata</rdfs:comment>
	</owl:Class>
	<owl:Class rdf:about="&j2se-1_4;JavaxImageioStreamAPI">
		<rdfs:subClassOf rdf:resource="&java;JavaAPI"/>
		<rdfs:comment xml:lang="en">JavaLibrary implementing the javax.imageio.stream package for J2SE 1.4</rdfs:comment>
		<rdfs:comment xml:lang="OWLManchester">platform:comprisesInterfacePart some JavaxImageioStream</rdfs:comment>
	</owl:Class>
	<owl:Class rdf:about="&j2se-1_4;JavaxImageioEventAPI">
		<rdfs:subClassOf rdf:resource="&java;JavaAPI"/>
		<rdfs:comment xml:lang="en">JavaLibrary implementing the javax.imageio.event package for J2SE 1.4</rdfs:comment>
		<rdfs:comment xml:lang="OWLManchester">platform:comprisesInterfacePart some JavaxImageioEvent</rdfs:comment>
	</owl:Class>
	<owl:Class rdf:about="&j2se-1_4;JavaxImageioPluginsJpegAPI">
		<rdfs:subClassOf rdf:resource="&java;JavaAPI"/>
		<rdfs:comment xml:lang="en">JavaLibrary implementing the javax.imageio.plugins.jpeg package for J2SE 1.4</rdfs:comment>
		<rdfs:comment xml:lang="OWLManchester">platform:comprisesInterfacePart some JavaxImageioPluginsJpeg</rdfs:comment>
	</owl:Class>
	<owl:Class rdf:about="&j2se-1_4;JavaxAccessibilityAPI">
		<rdfs:subClassOf rdf:resource="&j2se-1_3;JavaxAccessibilityAPI"/>
		<rdfs:comment xml:lang="en">JavaLibrary implementing the javax.accessibility package for J2SE 1.4</rdfs:comment>
		<rdfs:comment xml:lang="OWLManchester">platform:comprisesInterfacePart some JavaxAccessibility</rdfs:comment>
	</owl:Class>
	<owl:Class rdf:about="&j2se-1_4;JavaxSwingAPI">
		<rdfs:subClassOf rdf:resource="&java;JavaAPI"/>
		<rdfs:comment xml:lang="en">JavaLibrary implementing the javax.swing package for J2SE 1.4</rdfs:comment>
		<rdfs:comment xml:lang="OWLManchester">platform:comprisesInterfacePart some JavaxSwing</rdfs:comment>
	</owl:Class>
	<owl:Class rdf:about="&j2se-1_4;JavaxSwingPlafAPI">
		<rdfs:subClassOf rdf:resource="&j2se-1_3;JavaxSwingPlafAPI"/>
		<rdfs:comment xml:lang="en">JavaLibrary implementing the javax.swing.plaf package for J2SE 1.4</rdfs:comment>
		<rdfs:comment xml:lang="OWLManchester">platform:comprisesInterfacePart some JavaxSwingPlaf</rdfs:comment>
	</owl:Class>
	<owl:Class rdf:about="&j2se-1_4;JavaxSwingPlafBasicAPI">
		<rdfs:subClassOf rdf:resource="&j2se-1_3;JavaxSwingPlafBasicAPI"/>
		<rdfs:comment xml:lang="en">JavaLibrary implementing the javax.swing.plaf.basic package for J2SE 1.4</rdfs:comment>
		<rdfs:comment xml:lang="OWLManchester">platform:comprisesInterfacePart some JavaxSwingPlafBasic</rdfs:comment>
	</owl:Class>
	<owl:Class rdf:about="&j2se-1_4;JavaxSwingPlafMetalAPI">
		<rdfs:subClassOf rdf:resource="&j2se-1_3;JavaxSwingPlafMetalAPI"/>
		<rdfs:comment xml:lang="en">JavaLibrary implementing the javax.swing.plaf.metal package for J2SE 1.4</rdfs:comment>
		<rdfs:comment xml:lang="OWLManchester">platform:comprisesInterfacePart some JavaxSwingPlafMetal</rdfs:comment>
	</owl:Class>
	<owl:Class rdf:about="&j2se-1_4;JavaxSwingPlafMultiAPI">
		<rdfs:subClassOf rdf:resource="&j2se-1_3;JavaxSwingPlafMultiAPI"/>
		<rdfs:comment xml:lang="en">JavaLibrary implementing the javax.swing.plaf.multi package for J2SE 1.4</rdfs:comment>
		<rdfs:comment xml:lang="OWLManchester">platform:comprisesInterfacePart some JavaxSwingPlafMulti</rdfs:comment>
	</owl:Class>
	<owl:Class rdf:about="&j2se-1_4;JavaxSwingEventAPI">
		<rdfs:subClassOf rdf:resource="&j2se-1_3;JavaxSwingEventAPI"/>
		<rdfs:comment xml:lang="en">JavaLibrary implementing the javax.swing.event package for J2SE 1.4</rdfs:comment>
		<rdfs:comment xml:lang="OWLManchester">platform:comprisesInterfacePart some JavaxSwingEvent</rdfs:comment>
	</owl:Class>
	<owl:Class rdf:about="&j2se-1_4;JavaxSwingBorderAPI">
		<owl:equivalentClass rdf:resource="&j2se-1_3;JavaxSwingBorderAPI"/>
		<rdfs:subClassOf rdf:resource="&java;JavaAPI"/>
		<rdfs:comment xml:lang="en">JavaLibrary implementing the javax.swing.border package for J2SE 1.4</rdfs:comment>
		<rdfs:comment xml:lang="OWLManchester">platform:comprisesInterfacePart some JavaxSwingBorder</rdfs:comment>
	</owl:Class>
	<owl:Class rdf:about="&j2se-1_4;JavaxSwingTextAPI">
		<rdfs:subClassOf rdf:resource="&j2se-1_3;JavaxSwingTextAPI"/>
		<rdfs:comment xml:lang="en">JavaLibrary implementing the javax.swing.text package for J2SE 1.4</rdfs:comment>
		<rdfs:comment xml:lang="OWLManchester">platform:comprisesInterfacePart some JavaxSwingText</rdfs:comment>
	</owl:Class>
	<owl:Class rdf:about="&j2se-1_4;JavaxSwingTextHtmlAPI">
		<rdfs:subClassOf rdf:resource="&j2se-1_3;JavaxSwingTextHtmlAPI"/>
		<rdfs:comment xml:lang="en">JavaLibrary implementing the javax.swing.text.html package for J2SE 1.4</rdfs:comment>
		<rdfs:comment xml:lang="OWLManchester">platform:comprisesInterfacePart some JavaxSwingTextHtml</rdfs:comment>
	</owl:Class>
	<owl:Class rdf:about="&j2se-1_4;JavaxSwingTextHtmlParserAPI">
		<owl:equivalentClass rdf:resource="&j2se-1_3;JavaxSwingTextHtmlParserAPI"/>
		<rdfs:subClassOf rdf:resource="&java;JavaAPI"/>
		<rdfs:comment xml:lang="en">JavaLibrary implementing the javax.swing.text.html.parser package for J2SE 1.4</rdfs:comment>
		<rdfs:comment xml:lang="OWLManchester">platform:comprisesInterfacePart some JavaxSwingTextHtmlParser</rdfs:comment>
	</owl:Class>
	<owl:Class rdf:about="&j2se-1_4;JavaxSwingTextRtfAPI">
		<owl:equivalentClass rdf:resource="&j2se-1_3;JavaxSwingTextRtfAPI"/>
		<rdfs:subClassOf rdf:resource="&java;JavaAPI"/>
		<rdfs:comment xml:lang="en">JavaLibrary implementing the javax.swing.text.rtf package for J2SE 1.4</rdfs:comment>
		<rdfs:comment xml:lang="OWLManchester">platform:comprisesInterfacePart some JavaxSwingTextRtf</rdfs:comment>
	</owl:Class>
	<owl:Class rdf:about="&j2se-1_4;JavaxSwingTableAPI">
		<rdfs:subClassOf rdf:resource="&j2se-1_3;JavaxSwingTableAPI"/>
		<rdfs:comment xml:lang="en">JavaLibrary implementing the javax.swing.table package for J2SE 1.4</rdfs:comment>
		<rdfs:comment xml:lang="OWLManchester">platform:comprisesInterfacePart some JavaxSwingTable</rdfs:comment>
	</owl:Class>
	<owl:Class rdf:about="&j2se-1_4;JavaxSwingUndoAPI">
		<rdfs:subClassOf rdf:resource="&j2se-1_3;JavaxSwingUndoAPI"/>
		<rdfs:comment xml:lang="en">JavaLibrary implementing the javax.swing.undo package for J2SE 1.4</rdfs:comment>
		<rdfs:comment xml:lang="OWLManchester">platform:comprisesInterfacePart some JavaxSwingUndo</rdfs:comment>
	</owl:Class>
	<owl:Class rdf:about="&j2se-1_4;JavaxSwingTreeAPI">
		<rdfs:subClassOf rdf:resource="&j2se-1_3;JavaxSwingTreeAPI"/>
		<rdfs:comment xml:lang="en">JavaLibrary implementing the javax.swing.tree package for J2SE 1.4</rdfs:comment>
		<rdfs:comment xml:lang="OWLManchester">platform:comprisesInterfacePart some JavaxSwingTree</rdfs:comment>
	</owl:Class>
	<owl:Class rdf:about="&j2se-1_4;JavaxSwingFilechooserAPI">
		<rdfs:subClassOf rdf:resource="&j2se-1_3;JavaxSwingFilechooserAPI"/>
		<rdfs:comment xml:lang="en">JavaLibrary implementing the javax.swing.filechooser package for J2SE 1.4</rdfs:comment>
		<rdfs:comment xml:lang="OWLManchester">platform:comprisesInterfacePart some JavaxSwingFilechooser</rdfs:comment>
	</owl:Class>
	<owl:Class rdf:about="&j2se-1_4;JavaxSwingColorchooserAPI">
		<rdfs:subClassOf rdf:resource="&j2se-1_3;JavaxSwingColorchooserAPI"/>
		<rdfs:comment xml:lang="en">JavaLibrary implementing the javax.swing.colorchooser package for J2SE 1.4</rdfs:comment>
		<rdfs:comment xml:lang="OWLManchester">platform:comprisesInterfacePart some JavaxSwingColorchooser</rdfs:comment>
	</owl:Class>
	<owl:Class rdf:about="&j2se-1_4;JavaxSoundSampledAPI">
		<rdfs:subClassOf rdf:resource="&j2se-1_3;JavaxSoundSampledAPI"/>
		<rdfs:comment xml:lang="en">JavaLibrary implementing the javax.sound.sampled package for J2SE 1.4</rdfs:comment>
		<rdfs:comment xml:lang="OWLManchester">platform:comprisesInterfacePart some JavaxSoundSampled</rdfs:comment>
	</owl:Class>
	<owl:Class rdf:about="&j2se-1_4;JavaxSoundSampledSpiAPI">
		<owl:equivalentClass rdf:resource="&j2se-1_3;JavaxSoundSampledSpiAPI"/>
		<rdfs:subClassOf rdf:resource="&java;JavaAPI"/>
		<rdfs:comment xml:lang="en">JavaLibrary implementing the javax.sound.sampled.spi package for J2SE 1.4</rdfs:comment>
		<rdfs:comment xml:lang="OWLManchester">platform:comprisesInterfacePart some JavaxSoundSampledSpi</rdfs:comment>
	</owl:Class>
	<owl:Class rdf:about="&j2se-1_4;JavaxSoundMidiAPI">
		<rdfs:subClassOf rdf:resource="&j2se-1_3;JavaxSoundMidiAPI"/>
		<rdfs:comment xml:lang="en">JavaLibrary implementing the javax.sound.midi package for J2SE 1.4</rdfs:comment>
		<rdfs:comment xml:lang="OWLManchester">platform:comprisesInterfacePart some JavaxSoundMidi</rdfs:comment>
	</owl:Class>
	<owl:Class rdf:about="&j2se-1_4;JavaxSoundMidiSpiAPI">
		<owl:equivalentClass rdf:resource="&j2se-1_3;JavaxSoundMidiSpiAPI"/>
		<rdfs:subClassOf rdf:resource="&java;JavaAPI"/>
		<rdfs:comment xml:lang="en">JavaLibrary implementing the javax.sound.midi.spi package for J2SE 1.4</rdfs:comment>
		<rdfs:comment xml:lang="OWLManchester">platform:comprisesInterfacePart some JavaxSoundMidiSpi</rdfs:comment>
	</owl:Class>
	<owl:Class rdf:about="&j2se-1_4;JavaxPrintAPI">
		<rdfs:subClassOf rdf:resource="&java;JavaAPI"/>
		<rdfs:comment xml:lang="en">JavaLibrary implementing the javax.print package for J2SE 1.4</rdfs:comment>
		<rdfs:comment xml:lang="OWLManchester">platform:comprisesInterfacePart some JavaxPrint</rdfs:comment>
	</owl:Class>
	<owl:Class rdf:about="&j2se-1_4;JavaxPrintAttributeAPI">
		<rdfs:subClassOf rdf:resource="&java;JavaAPI"/>
		<rdfs:comment xml:lang="en">JavaLibrary implementing the javax.print.attribute package for J2SE 1.4</rdfs:comment>
		<rdfs:comment xml:lang="OWLManchester">platform:comprisesInterfacePart some JavaxPrintAttribute</rdfs:comment>
	</owl:Class>
	<owl:Class rdf:about="&j2se-1_4;JavaxPrintAttributeStandardAPI">
		<rdfs:subClassOf rdf:resource="&java;JavaAPI"/>
		<rdfs:comment xml:lang="en">JavaLibrary implementing the javax.print.attribute.standard package for J2SE 1.4</rdfs:comment>
		<rdfs:comment xml:lang="OWLManchester">platform:comprisesInterfacePart some JavaxPrintAttributeStandard</rdfs:comment>
	</owl:Class>
	<owl:Class rdf:about="&j2se-1_4;JavaxPrintEventAPI">
		<rdfs:subClassOf rdf:resource="&java;JavaAPI"/>
		<rdfs:comment xml:lang="en">JavaLibrary implementing the javax.print.event package for J2SE 1.4</rdfs:comment>
		<rdfs:comment xml:lang="OWLManchester">platform:comprisesInterfacePart some JavaxPrintEvent</rdfs:comment>
	</owl:Class>
	<owl:Class rdf:about="&j2se-1_4;JavaxSecurityAuthAPI">
		<rdfs:subClassOf rdf:resource="&java;JavaAPI"/>
		<rdfs:comment xml:lang="en">JavaLibrary implementing the javax.security.auth package for J2SE 1.4</rdfs:comment>
		<rdfs:comment xml:lang="OWLManchester">platform:comprisesInterfacePart some JavaxSecurityAuth</rdfs:comment>
	</owl:Class>
	<owl:Class rdf:about="&j2se-1_4;JavaxSecurityAuthX500API">
		<rdfs:subClassOf rdf:resource="&j2me-pp-1_1;JavaxSecurityAuthX500API"/>
		<rdfs:comment xml:lang="en">JavaLibrary implementing the javax.security.auth.x500 package for J2SE 1.4</rdfs:comment>
		<rdfs:comment xml:lang="OWLManchester">platform:comprisesInterfacePart some JavaxSecurityAuthX500</rdfs:comment>
	</owl:Class>
	<owl:Class rdf:about="&j2se-1_4;JavaxSecurityAuthCallbackAPI">
		<rdfs:subClassOf rdf:resource="&java;JavaAPI"/>
		<rdfs:comment xml:lang="en">JavaLibrary implementing the javax.security.auth.callback package for J2SE 1.4</rdfs:comment>
		<rdfs:comment xml:lang="OWLManchester">platform:comprisesInterfacePart some JavaxSecurityAuthCallback</rdfs:comment>
	</owl:Class>
	<owl:Class rdf:about="&j2se-1_4;JavaxSecurityAuthKerberosAPI">
		<rdfs:subClassOf rdf:resource="&java;JavaAPI"/>
		<rdfs:comment xml:lang="en">JavaLibrary implementing the javax.security.auth.kerberos package for J2SE 1.4</rdfs:comment>
		<rdfs:comment xml:lang="OWLManchester">platform:comprisesInterfacePart some JavaxSecurityAuthKerberos</rdfs:comment>
	</owl:Class>
	<owl:Class rdf:about="&j2se-1_4;JavaxSecurityAuthLoginAPI">
		<rdfs:subClassOf rdf:resource="&java;JavaAPI"/>
		<rdfs:comment xml:lang="en">JavaLibrary implementing the javax.security.auth.login package for J2SE 1.4</rdfs:comment>
		<rdfs:comment xml:lang="OWLManchester">platform:comprisesInterfacePart some JavaxSecurityAuthLogin</rdfs:comment>
	</owl:Class>
	<owl:Class rdf:about="&j2se-1_4;JavaxSecurityAuthSpiAPI">
		<rdfs:subClassOf rdf:resource="&java;JavaAPI"/>
		<rdfs:comment xml:lang="en">JavaLibrary implementing the javax.security.auth.spi package for J2SE 1.4</rdfs:comment>
		<rdfs:comment xml:lang="OWLManchester">platform:comprisesInterfacePart some JavaxSecurityAuthSpi</rdfs:comment>
	</owl:Class>
	<owl:Class rdf:about="&j2se-1_4;JavaxSecurityCertAPI">
		<rdfs:subClassOf rdf:resource="&java;JavaAPI"/>
		<rdfs:comment xml:lang="en">JavaLibrary implementing the javax.security.cert package for J2SE 1.4</rdfs:comment>
		<rdfs:comment xml:lang="OWLManchester">platform:comprisesInterfacePart some JavaxSecurityCert</rdfs:comment>
	</owl:Class>
	<owl:Class rdf:about="&j2se-1_4;JavaxNamingAPI">
		<rdfs:subClassOf rdf:resource="&j2se-1_3;JavaxNamingAPI"/>
		<rdfs:comment xml:lang="en">JavaLibrary implementing the javax.naming package for J2SE 1.4</rdfs:comment>
		<rdfs:comment xml:lang="OWLManchester">platform:comprisesInterfacePart some JavaxNaming</rdfs:comment>
	</owl:Class>
	<owl:Class rdf:about="&j2se-1_4;JavaxNamingDirectoryAPI">
		<rdfs:subClassOf rdf:resource="&j2se-1_3;JavaxNamingDirectoryAPI"/>
		<rdfs:comment xml:lang="en">JavaLibrary implementing the javax.naming.directory package for J2SE 1.4</rdfs:comment>
		<rdfs:comment xml:lang="OWLManchester">platform:comprisesInterfacePart some JavaxNamingDirectory</rdfs:comment>
	</owl:Class>
	<owl:Class rdf:about="&j2se-1_4;JavaxNamingEventAPI">
		<owl:equivalentClass rdf:resource="&j2se-1_3;JavaxNamingEventAPI"/>
		<rdfs:subClassOf rdf:resource="&java;JavaAPI"/>
		<rdfs:comment xml:lang="en">JavaLibrary implementing the javax.naming.event package for J2SE 1.4</rdfs:comment>
		<rdfs:comment xml:lang="OWLManchester">platform:comprisesInterfacePart some JavaxNamingEvent</rdfs:comment>
	</owl:Class>
	<owl:Class rdf:about="&j2se-1_4;JavaxNamingLdapAPI">
		<rdfs:subClassOf rdf:resource="&j2se-1_3;JavaxNamingLdapAPI"/>
		<rdfs:comment xml:lang="en">JavaLibrary implementing the javax.naming.ldap package for J2SE 1.4</rdfs:comment>
		<rdfs:comment xml:lang="OWLManchester">platform:comprisesInterfacePart some JavaxNamingLdap</rdfs:comment>
	</owl:Class>
	<owl:Class rdf:about="&j2se-1_4;JavaxNamingSpiAPI">
		<owl:equivalentClass rdf:resource="&j2se-1_3;JavaxNamingSpiAPI"/>
		<rdfs:subClassOf rdf:resource="&java;JavaAPI"/>
		<rdfs:comment xml:lang="en">JavaLibrary implementing the javax.naming.spi package for J2SE 1.4</rdfs:comment>
		<rdfs:comment xml:lang="OWLManchester">platform:comprisesInterfacePart some JavaxNamingSpi</rdfs:comment>
	</owl:Class>
	<owl:Class rdf:about="&j2se-1_4;JavaxNetAPI">
		<rdfs:subClassOf rdf:resource="&java;JavaAPI"/>
		<rdfs:comment xml:lang="en">JavaLibrary implementing the javax.net package for J2SE 1.4</rdfs:comment>
		<rdfs:comment xml:lang="OWLManchester">platform:comprisesInterfacePart some JavaxNet</rdfs:comment>
	</owl:Class>
	<owl:Class rdf:about="&j2se-1_4;JavaxNetSslAPI">
		<rdfs:subClassOf rdf:resource="&java;JavaAPI"/>
		<rdfs:comment xml:lang="en">JavaLibrary implementing the javax.net.ssl package for J2SE 1.4</rdfs:comment>
		<rdfs:comment xml:lang="OWLManchester">platform:comprisesInterfacePart some JavaxNetSsl</rdfs:comment>
	</owl:Class>
	<owl:Class rdf:about="&j2se-1_4;JavaxRmiAPI">
		<owl:equivalentClass rdf:resource="&j2se-1_3;JavaxRmiAPI"/>
		<rdfs:subClassOf rdf:resource="&java;JavaAPI"/>
		<rdfs:comment xml:lang="en">JavaLibrary implementing the javax.rmi package for J2SE 1.4</rdfs:comment>
		<rdfs:comment xml:lang="OWLManchester">platform:comprisesInterfacePart some JavaxRmi</rdfs:comment>
	</owl:Class>
	<owl:Class rdf:about="&j2se-1_4;JavaxRmiCORBAAPI">
		<owl:equivalentClass rdf:resource="&j2se-1_3;JavaxRmiCORBAAPI"/>
		<rdfs:subClassOf rdf:resource="&java;JavaAPI"/>
		<rdfs:comment xml:lang="en">JavaLibrary implementing the javax.rmi.CORBA package for J2SE 1.4</rdfs:comment>
		<rdfs:comment xml:lang="OWLManchester">platform:comprisesInterfacePart some JavaxRmiCORBA</rdfs:comment>
	</owl:Class>
	<owl:Class rdf:about="&j2se-1_4;JavaxCryptoAPI">
		<rdfs:subClassOf rdf:resource="&java;JavaAPI"/>
		<rdfs:comment xml:lang="en">JavaLibrary implementing the javax.crypto package for J2SE 1.4</rdfs:comment>
		<rdfs:comment xml:lang="OWLManchester">platform:comprisesInterfacePart some JavaxCrypto</rdfs:comment>
	</owl:Class>
	<owl:Class rdf:about="&j2se-1_4;JavaxCryptoInterfacesAPI">
		<rdfs:subClassOf rdf:resource="&java;JavaAPI"/>
		<rdfs:comment xml:lang="en">JavaLibrary implementing the javax.crypto.interfaces package for J2SE 1.4</rdfs:comment>
		<rdfs:comment xml:lang="OWLManchester">platform:comprisesInterfacePart some JavaxCryptoInterfaces</rdfs:comment>
	</owl:Class>
	<owl:Class rdf:about="&j2se-1_4;JavaxCryptoSpecAPI">
		<rdfs:subClassOf rdf:resource="&java;JavaAPI"/>
		<rdfs:comment xml:lang="en">JavaLibrary implementing the javax.crypto.spec package for J2SE 1.4</rdfs:comment>
		<rdfs:comment xml:lang="OWLManchester">platform:comprisesInterfacePart some JavaxCryptoSpec</rdfs:comment>
	</owl:Class>
	<owl:Class rdf:about="&j2se-1_4;JavaxSqlAPI">
		<rdfs:subClassOf rdf:resource="&java;JavaAPI"/>
		<rdfs:comment xml:lang="en">JavaLibrary implementing the javax.sql package for J2SE 1.4</rdfs:comment>
		<rdfs:comment xml:lang="OWLManchester">platform:comprisesInterfacePart some JavaxSql</rdfs:comment>
	</owl:Class>
	<owl:Class rdf:about="&j2se-1_4;JavaxTransactionAPI">
		<rdfs:subClassOf rdf:resource="&j2se-1_3;JavaxTransactionAPI"/>
		<rdfs:comment xml:lang="en">JavaLibrary implementing the javax.transaction package for J2SE 1.4</rdfs:comment>
		<rdfs:comment xml:lang="OWLManchester">platform:comprisesInterfacePart some JavaxTransaction</rdfs:comment>
	</owl:Class>
	<owl:Class rdf:about="&j2se-1_4;JavaxTransactionXaAPI">
		<rdfs:subClassOf rdf:resource="&java;JavaAPI"/>
		<rdfs:comment xml:lang="en">JavaLibrary implementing the javax.transaction.xa package for J2SE 1.4</rdfs:comment>
		<rdfs:comment xml:lang="OWLManchester">platform:comprisesInterfacePart some JavaxTransactionXa</rdfs:comment>
	</owl:Class>
	<owl:Class rdf:about="&j2se-1_4;JavaxXmlParsersAPI">
		<rdfs:subClassOf rdf:resource="&java;JavaAPI"/>
		<rdfs:comment xml:lang="en">JavaLibrary implementing the javax.xml.parsers package for J2SE 1.4</rdfs:comment>
		<rdfs:comment xml:lang="OWLManchester">platform:comprisesInterfacePart some JavaxXmlParsers</rdfs:comment>
	</owl:Class>
	<owl:Class rdf:about="&j2se-1_4;JavaxXmlTransformAPI">
		<rdfs:subClassOf rdf:resource="&java;JavaAPI"/>
		<rdfs:comment xml:lang="en">JavaLibrary implementing the javax.xml.transform package for J2SE 1.4</rdfs:comment>
		<rdfs:comment xml:lang="OWLManchester">platform:comprisesInterfacePart some JavaxXmlTransform</rdfs:comment>
	</owl:Class>
	<owl:Class rdf:about="&j2se-1_4;JavaxXmlTransformDomAPI">
		<rdfs:subClassOf rdf:resource="&java;JavaAPI"/>
		<rdfs:comment xml:lang="en">JavaLibrary implementing the javax.xml.transform.dom package for J2SE 1.4</rdfs:comment>
		<rdfs:comment xml:lang="OWLManchester">platform:comprisesInterfacePart some JavaxXmlTransformDom</rdfs:comment>
	</owl:Class>
	<owl:Class rdf:about="&j2se-1_4;JavaxXmlTransformSaxAPI">
		<rdfs:subClassOf rdf:resource="&java;JavaAPI"/>
		<rdfs:comment xml:lang="en">JavaLibrary implementing the javax.xml.transform.sax package for J2SE 1.4</rdfs:comment>
		<rdfs:comment xml:lang="OWLManchester">platform:comprisesInterfacePart some JavaxXmlTransformSax</rdfs:comment>
	</owl:Class>
	<owl:Class rdf:about="&j2se-1_4;JavaxXmlTransformStreamAPI">
		<rdfs:subClassOf rdf:resource="&java;JavaAPI"/>
		<rdfs:comment xml:lang="en">JavaLibrary implementing the javax.xml.transform.stream package for J2SE 1.4</rdfs:comment>
		<rdfs:comment xml:lang="OWLManchester">platform:comprisesInterfacePart some JavaxXmlTransformStream</rdfs:comment>
	</owl:Class>
	<owl:Class rdf:about="&j2se-1_4;OrgW3cDomAPI">
		<rdfs:subClassOf rdf:resource="&java;JavaAPI"/>
		<rdfs:comment xml:lang="en">JavaLibrary implementing the org.w3c.dom package for J2SE 1.4</rdfs:comment>
		<rdfs:comment xml:lang="OWLManchester">platform:comprisesInterfacePart some OrgW3cDom</rdfs:comment>
	</owl:Class>
	<owl:Class rdf:about="&j2se-1_4;OrgW3cDomCssAPI">
		<rdfs:subClassOf rdf:resource="&java;JavaAPI"/>
		<rdfs:comment xml:lang="en">JavaLibrary implementing the org.w3c.dom.css package for J2SE 1.4</rdfs:comment>
		<rdfs:comment xml:lang="OWLManchester">platform:comprisesInterfacePart some OrgW3cDomCss</rdfs:comment>
	</owl:Class>
	<owl:Class rdf:about="&j2se-1_4;OrgW3cDomStylesheetsAPI">
		<rdfs:subClassOf rdf:resource="&java;JavaAPI"/>
		<rdfs:comment xml:lang="en">JavaLibrary implementing the org.w3c.dom.stylesheets package for J2SE 1.4</rdfs:comment>
		<rdfs:comment xml:lang="OWLManchester">platform:comprisesInterfacePart some OrgW3cDomStylesheets</rdfs:comment>
	</owl:Class>
	<owl:Class rdf:about="&j2se-1_4;OrgW3cDomViewsAPI">
		<rdfs:subClassOf rdf:resource="&java;JavaAPI"/>
		<rdfs:comment xml:lang="en">JavaLibrary implementing the org.w3c.dom.views package for J2SE 1.4</rdfs:comment>
		<rdfs:comment xml:lang="OWLManchester">platform:comprisesInterfacePart some OrgW3cDomViews</rdfs:comment>
	</owl:Class>
	<owl:Class rdf:about="&j2se-1_4;OrgW3cDomEventsAPI">
		<rdfs:subClassOf rdf:resource="&java;JavaAPI"/>
		<rdfs:comment xml:lang="en">JavaLibrary implementing the org.w3c.dom.events package for J2SE 1.4</rdfs:comment>
		<rdfs:comment xml:lang="OWLManchester">platform:comprisesInterfacePart some OrgW3cDomEvents</rdfs:comment>
	</owl:Class>
	<owl:Class rdf:about="&j2se-1_4;OrgW3cDomHtmlAPI">
		<rdfs:subClassOf rdf:resource="&java;JavaAPI"/>
		<rdfs:comment xml:lang="en">JavaLibrary implementing the org.w3c.dom.html package for J2SE 1.4</rdfs:comment>
		<rdfs:comment xml:lang="OWLManchester">platform:comprisesInterfacePart some OrgW3cDomHtml</rdfs:comment>
	</owl:Class>
	<owl:Class rdf:about="&j2se-1_4;OrgW3cDomTraversalAPI">
		<rdfs:subClassOf rdf:resource="&java;JavaAPI"/>
		<rdfs:comment xml:lang="en">JavaLibrary implementing the org.w3c.dom.traversal package for J2SE 1.4</rdfs:comment>
		<rdfs:comment xml:lang="OWLManchester">platform:comprisesInterfacePart some OrgW3cDomTraversal</rdfs:comment>
	</owl:Class>
	<owl:Class rdf:about="&j2se-1_4;OrgOmgCORBA_2_3API">
		<owl:equivalentClass rdf:resource="&j2se-1_3;OrgOmgCORBA_2_3API"/>
		<rdfs:subClassOf rdf:resource="&java;JavaAPI"/>
		<rdfs:comment xml:lang="en">JavaLibrary implementing the org.omg.CORBA_2_3 package for J2SE 1.4</rdfs:comment>
		<rdfs:comment xml:lang="OWLManchester">platform:comprisesInterfacePart some OrgOmgCORBA_2_3</rdfs:comment>
	</owl:Class>
	<owl:Class rdf:about="&j2se-1_4;OrgOmgCORBA_2_3PortableAPI">
		<rdfs:subClassOf rdf:resource="&java;JavaAPI"/>
		<rdfs:comment xml:lang="en">JavaLibrary implementing the org.omg.CORBA_2_3.portable package for J2SE 1.4</rdfs:comment>
		<rdfs:comment xml:lang="OWLManchester">platform:comprisesInterfacePart some OrgOmgCORBA_2_3Portable</rdfs:comment>
	</owl:Class>
	<owl:Class rdf:about="&j2se-1_4;OrgOmgCORBAAPI">
		<rdfs:subClassOf rdf:resource="&java;JavaAPI"/>
		<rdfs:comment xml:lang="en">JavaLibrary implementing the org.omg.CORBA package for J2SE 1.4</rdfs:comment>
		<rdfs:comment xml:lang="OWLManchester">platform:comprisesInterfacePart some OrgOmgCORBA</rdfs:comment>
	</owl:Class>
	<owl:Class rdf:about="&j2se-1_4;OrgOmgCORBAPortableAPI">
		<rdfs:subClassOf rdf:resource="&java;JavaAPI"/>
		<rdfs:comment xml:lang="en">JavaLibrary implementing the org.omg.CORBA.portable package for J2SE 1.4</rdfs:comment>
		<rdfs:comment xml:lang="OWLManchester">platform:comprisesInterfacePart some OrgOmgCORBAPortable</rdfs:comment>
	</owl:Class>
	<owl:Class rdf:about="&j2se-1_4;OrgOmgCORBADynAnyPackageAPI">
		<rdfs:subClassOf rdf:resource="&j2se-1_3;OrgOmgCORBADynAnyPackageAPI"/>
		<rdfs:comment xml:lang="en">JavaLibrary implementing the org.omg.CORBA.DynAnyPackage package for J2SE 1.4</rdfs:comment>
		<rdfs:comment xml:lang="OWLManchester">platform:comprisesInterfacePart some OrgOmgCORBADynAnyPackage</rdfs:comment>
	</owl:Class>
	<owl:Class rdf:about="&j2se-1_4;OrgOmgCORBAORBPackageAPI">
		<rdfs:subClassOf rdf:resource="&j2se-1_3;OrgOmgCORBAORBPackageAPI"/>
		<rdfs:comment xml:lang="en">JavaLibrary implementing the org.omg.CORBA.ORBPackage package for J2SE 1.4</rdfs:comment>
		<rdfs:comment xml:lang="OWLManchester">platform:comprisesInterfacePart some OrgOmgCORBAORBPackage</rdfs:comment>
	</owl:Class>
	<owl:Class rdf:about="&j2se-1_4;OrgOmgCORBATypeCodePackageAPI">
		<rdfs:subClassOf rdf:resource="&j2se-1_3;OrgOmgCORBATypeCodePackageAPI"/>
		<rdfs:comment xml:lang="en">JavaLibrary implementing the org.omg.CORBA.TypeCodePackage package for J2SE 1.4</rdfs:comment>
		<rdfs:comment xml:lang="OWLManchester">platform:comprisesInterfacePart some OrgOmgCORBATypeCodePackage</rdfs:comment>
	</owl:Class>
	<owl:Class rdf:about="&j2se-1_4;OrgOmgSendingContextAPI">
		<owl:equivalentClass rdf:resource="&j2se-1_3;OrgOmgSendingContextAPI"/>
		<rdfs:subClassOf rdf:resource="&java;JavaAPI"/>
		<rdfs:comment xml:lang="en">JavaLibrary implementing the org.omg.SendingContext package for J2SE 1.4</rdfs:comment>
		<rdfs:comment xml:lang="OWLManchester">platform:comprisesInterfacePart some OrgOmgSendingContext</rdfs:comment>
	</owl:Class>
	<owl:Class rdf:about="&j2se-1_4;OrgOmgCosNamingAPI">
		<rdfs:subClassOf rdf:resource="&java;JavaAPI"/>
		<rdfs:comment xml:lang="en">JavaLibrary implementing the org.omg.CosNaming package for J2SE 1.4</rdfs:comment>
		<rdfs:comment xml:lang="OWLManchester">platform:comprisesInterfacePart some OrgOmgCosNaming</rdfs:comment>
	</owl:Class>
	<owl:Class rdf:about="&j2se-1_4;OrgOmgCosNamingNamingContextExtPackageAPI">
		<rdfs:subClassOf rdf:resource="&java;JavaAPI"/>
		<rdfs:comment xml:lang="en">JavaLibrary implementing the org.omg.CosNaming.NamingContextExtPackage package for J2SE 1.4</rdfs:comment>
		<rdfs:comment xml:lang="OWLManchester">platform:comprisesInterfacePart some OrgOmgCosNamingNamingContextExtPackage</rdfs:comment>
	</owl:Class>
	<owl:Class rdf:about="&j2se-1_4;OrgOmgCosNamingNamingContextPackageAPI">
		<rdfs:subClassOf rdf:resource="&java;JavaAPI"/>
		<rdfs:comment xml:lang="en">JavaLibrary implementing the org.omg.CosNaming.NamingContextPackage package for J2SE 1.4</rdfs:comment>
		<rdfs:comment xml:lang="OWLManchester">platform:comprisesInterfacePart some OrgOmgCosNamingNamingContextPackage</rdfs:comment>
	</owl:Class>
	<owl:Class rdf:about="&j2se-1_4;OrgOmgPortableServerAPI">
		<rdfs:subClassOf rdf:resource="&java;JavaAPI"/>
		<rdfs:comment xml:lang="en">JavaLibrary implementing the org.omg.PortableServer package for J2SE 1.4</rdfs:comment>
		<rdfs:comment xml:lang="OWLManchester">platform:comprisesInterfacePart some OrgOmgPortableServer</rdfs:comment>
	</owl:Class>
	<owl:Class rdf:about="&j2se-1_4;OrgOmgPortableServerCurrentPackageAPI">
		<rdfs:subClassOf rdf:resource="&java;JavaAPI"/>
		<rdfs:comment xml:lang="en">JavaLibrary implementing the org.omg.PortableServer.CurrentPackage package for J2SE 1.4</rdfs:comment>
		<rdfs:comment xml:lang="OWLManchester">platform:comprisesInterfacePart some OrgOmgPortableServerCurrentPackage</rdfs:comment>
	</owl:Class>
	<owl:Class rdf:about="&j2se-1_4;OrgOmgPortableServerPOAManagerPackageAPI">
		<rdfs:subClassOf rdf:resource="&java;JavaAPI"/>
		<rdfs:comment xml:lang="en">JavaLibrary implementing the org.omg.PortableServer.POAManagerPackage package for J2SE 1.4</rdfs:comment>
		<rdfs:comment xml:lang="OWLManchester">platform:comprisesInterfacePart some OrgOmgPortableServerPOAManagerPackage</rdfs:comment>
	</owl:Class>
	<owl:Class rdf:about="&j2se-1_4;OrgOmgPortableServerPOAPackageAPI">
		<rdfs:subClassOf rdf:resource="&java;JavaAPI"/>
		<rdfs:comment xml:lang="en">JavaLibrary implementing the org.omg.PortableServer.POAPackage package for J2SE 1.4</rdfs:comment>
		<rdfs:comment xml:lang="OWLManchester">platform:comprisesInterfacePart some OrgOmgPortableServerPOAPackage</rdfs:comment>
	</owl:Class>
	<owl:Class rdf:about="&j2se-1_4;OrgOmgPortableServerPortableAPI">
		<rdfs:subClassOf rdf:resource="&java;JavaAPI"/>
		<rdfs:comment xml:lang="en">JavaLibrary implementing the org.omg.PortableServer.portable package for J2SE 1.4</rdfs:comment>
		<rdfs:comment xml:lang="OWLManchester">platform:comprisesInterfacePart some OrgOmgPortableServerPortable</rdfs:comment>
	</owl:Class>
	<owl:Class rdf:about="&j2se-1_4;OrgOmgPortableServerServantLocatorPackageAPI">
		<rdfs:subClassOf rdf:resource="&java;JavaAPI"/>
		<rdfs:comment xml:lang="en">JavaLibrary implementing the org.omg.PortableServer.ServantLocatorPackage package for J2SE 1.4</rdfs:comment>
		<rdfs:comment xml:lang="OWLManchester">platform:comprisesInterfacePart some OrgOmgPortableServerServantLocatorPackage</rdfs:comment>
	</owl:Class>
	<owl:Class rdf:about="&j2se-1_4;OrgOmgDynamicAPI">
		<rdfs:subClassOf rdf:resource="&java;JavaAPI"/>
		<rdfs:comment xml:lang="en">JavaLibrary implementing the org.omg.Dynamic package for J2SE 1.4</rdfs:comment>
		<rdfs:comment xml:lang="OWLManchester">platform:comprisesInterfacePart some OrgOmgDynamic</rdfs:comment>
	</owl:Class>
	<owl:Class rdf:about="&j2se-1_4;OrgOmgDynamicAnyAPI">
		<rdfs:subClassOf rdf:resource="&java;JavaAPI"/>
		<rdfs:comment xml:lang="en">JavaLibrary implementing the org.omg.DynamicAny package for J2SE 1.4</rdfs:comment>
		<rdfs:comment xml:lang="OWLManchester">platform:comprisesInterfacePart some OrgOmgDynamicAny</rdfs:comment>
	</owl:Class>
	<owl:Class rdf:about="&j2se-1_4;OrgOmgDynamicAnyDynAnyFactoryPackageAPI">
		<rdfs:subClassOf rdf:resource="&java;JavaAPI"/>
		<rdfs:comment xml:lang="en">JavaLibrary implementing the org.omg.DynamicAny.DynAnyFactoryPackage package for J2SE 1.4</rdfs:comment>
		<rdfs:comment xml:lang="OWLManchester">platform:comprisesInterfacePart some OrgOmgDynamicAnyDynAnyFactoryPackage</rdfs:comment>
	</owl:Class>
	<owl:Class rdf:about="&j2se-1_4;OrgOmgDynamicAnyDynAnyPackageAPI">
		<rdfs:subClassOf rdf:resource="&java;JavaAPI"/>
		<rdfs:comment xml:lang="en">JavaLibrary implementing the org.omg.DynamicAny.DynAnyPackage package for J2SE 1.4</rdfs:comment>
		<rdfs:comment xml:lang="OWLManchester">platform:comprisesInterfacePart some OrgOmgDynamicAnyDynAnyPackage</rdfs:comment>
	</owl:Class>
	<owl:Class rdf:about="&j2se-1_4;OrgOmgIOPAPI">
		<rdfs:subClassOf rdf:resource="&java;JavaAPI"/>
		<rdfs:comment xml:lang="en">JavaLibrary implementing the org.omg.IOP package for J2SE 1.4</rdfs:comment>
		<rdfs:comment xml:lang="OWLManchester">platform:comprisesInterfacePart some OrgOmgIOP</rdfs:comment>
	</owl:Class>
	<owl:Class rdf:about="&j2se-1_4;OrgOmgIOPCodecFactoryPackageAPI">
		<rdfs:subClassOf rdf:resource="&java;JavaAPI"/>
		<rdfs:comment xml:lang="en">JavaLibrary implementing the org.omg.IOP.CodecFactoryPackage package for J2SE 1.4</rdfs:comment>
		<rdfs:comment xml:lang="OWLManchester">platform:comprisesInterfacePart some OrgOmgIOPCodecFactoryPackage</rdfs:comment>
	</owl:Class>
	<owl:Class rdf:about="&j2se-1_4;OrgOmgIOPCodecPackageAPI">
		<rdfs:subClassOf rdf:resource="&java;JavaAPI"/>
		<rdfs:comment xml:lang="en">JavaLibrary implementing the org.omg.IOP.CodecPackage package for J2SE 1.4</rdfs:comment>
		<rdfs:comment xml:lang="OWLManchester">platform:comprisesInterfacePart some OrgOmgIOPCodecPackage</rdfs:comment>
	</owl:Class>
	<owl:Class rdf:about="&j2se-1_4;OrgOmgMessagingAPI">
		<rdfs:subClassOf rdf:resource="&java;JavaAPI"/>
		<rdfs:comment xml:lang="en">JavaLibrary implementing the org.omg.Messaging package for J2SE 1.4</rdfs:comment>
		<rdfs:comment xml:lang="OWLManchester">platform:comprisesInterfacePart some OrgOmgMessaging</rdfs:comment>
	</owl:Class>
	<owl:Class rdf:about="&j2se-1_4;OrgOmgPortableInterceptorAPI">
		<rdfs:subClassOf rdf:resource="&java;JavaAPI"/>
		<rdfs:comment xml:lang="en">JavaLibrary implementing the org.omg.PortableInterceptor package for J2SE 1.4</rdfs:comment>
		<rdfs:comment xml:lang="OWLManchester">platform:comprisesInterfacePart some OrgOmgPortableInterceptor</rdfs:comment>
	</owl:Class>
	<owl:Class rdf:about="&j2se-1_4;OrgOmgPortableInterceptorORBInitInfoPackageAPI">
		<rdfs:subClassOf rdf:resource="&java;JavaAPI"/>
		<rdfs:comment xml:lang="en">JavaLibrary implementing the org.omg.PortableInterceptor.ORBInitInfoPackage package for J2SE 1.4</rdfs:comment>
		<rdfs:comment xml:lang="OWLManchester">platform:comprisesInterfacePart some OrgOmgPortableInterceptorORBInitInfoPackage</rdfs:comment>
	</owl:Class>
	<owl:Class rdf:about="&j2se-1_4;OrgOmgStubJavaRmiAPI">
		<owl:equivalentClass rdf:resource="&j2se-1_3;OrgOmgStubJavaRmiAPI"/>
		<rdfs:subClassOf rdf:resource="&java;JavaAPI"/>
		<rdfs:comment xml:lang="en">JavaLibrary implementing the org.omg.stub.java.rmi package for J2SE 1.4</rdfs:comment>
		<rdfs:comment xml:lang="OWLManchester">platform:comprisesInterfacePart some OrgOmgStubJavaRmi</rdfs:comment>
	</owl:Class>
	<owl:Class rdf:about="&j2se-1_4;OrgXmlSaxAPI">
		<rdfs:subClassOf rdf:resource="&java;JavaAPI"/>
		<rdfs:comment xml:lang="en">JavaLibrary implementing the org.xml.sax package for J2SE 1.4</rdfs:comment>
		<rdfs:comment xml:lang="OWLManchester">platform:comprisesInterfacePart some OrgXmlSax</rdfs:comment>
	</owl:Class>
	<owl:Class rdf:about="&j2se-1_4;OrgXmlSaxHelpersAPI">
		<rdfs:subClassOf rdf:resource="&java;JavaAPI"/>
		<rdfs:comment xml:lang="en">JavaLibrary implementing the org.xml.sax.helpers package for J2SE 1.4</rdfs:comment>
		<rdfs:comment xml:lang="OWLManchester">platform:comprisesInterfacePart some OrgXmlSaxHelpers</rdfs:comment>
	</owl:Class>
	<owl:Class rdf:about="&j2se-1_4;OrgXmlSaxExtAPI">
		<rdfs:subClassOf rdf:resource="&java;JavaAPI"/>
		<rdfs:comment xml:lang="en">JavaLibrary implementing the org.xml.sax.ext package for J2SE 1.4</rdfs:comment>
		<rdfs:comment xml:lang="OWLManchester">platform:comprisesInterfacePart some OrgXmlSaxExt</rdfs:comment>
	</owl:Class>
	<owl:Class rdf:about="&j2se-1_4;OrgIetfJgssAPI">
		<rdfs:subClassOf rdf:resource="&java;JavaAPI"/>
		<rdfs:comment xml:lang="en">JavaLibrary implementing the org.ietf.jgss package for J2SE 1.4</rdfs:comment>
		<rdfs:comment xml:lang="OWLManchester">platform:comprisesInterfacePart some OrgIetfJgss</rdfs:comment>
	</owl:Class>
	<j2se-1_4:JavaLang rdf:about="&j2se-1_4;theJavaLangPart">
	</j2se-1_4:JavaLang>
	<j2se-1_4:JavaLangReflect rdf:about="&j2se-1_4;theJavaLangReflectPart">
	</j2se-1_4:JavaLangReflect>
	<j2se-1_4:JavaLangRef rdf:about="&j2se-1_4;theJavaLangRefPart">
	</j2se-1_4:JavaLangRef>
	<j2se-1_4:JavaIo rdf:about="&j2se-1_4;theJavaIoPart">
	</j2se-1_4:JavaIo>
	<j2se-1_4:JavaUtil rdf:about="&j2se-1_4;theJavaUtilPart">
	</j2se-1_4:JavaUtil>
	<j2se-1_4:JavaUtilLogging rdf:about="&j2se-1_4;theJavaUtilLoggingPart">
	</j2se-1_4:JavaUtilLogging>
	<j2se-1_4:JavaUtilJar rdf:about="&j2se-1_4;theJavaUtilJarPart">
	</j2se-1_4:JavaUtilJar>
	<j2se-1_4:JavaUtilZip rdf:about="&j2se-1_4;theJavaUtilZipPart">
	</j2se-1_4:JavaUtilZip>
	<j2se-1_4:JavaUtilPrefs rdf:about="&j2se-1_4;theJavaUtilPrefsPart">
	</j2se-1_4:JavaUtilPrefs>
	<j2se-1_4:JavaUtilRegex rdf:about="&j2se-1_4;theJavaUtilRegexPart">
	</j2se-1_4:JavaUtilRegex>
	<j2se-1_4:JavaNet rdf:about="&j2se-1_4;theJavaNetPart">
	</j2se-1_4:JavaNet>
	<j2se-1_4:JavaSecurity rdf:about="&j2se-1_4;theJavaSecurityPart">
	</j2se-1_4:JavaSecurity>
	<j2se-1_4:JavaSecurityCert rdf:about="&j2se-1_4;theJavaSecurityCertPart">
	</j2se-1_4:JavaSecurityCert>
	<j2se-1_4:JavaSecuritySpec rdf:about="&j2se-1_4;theJavaSecuritySpecPart">
	</j2se-1_4:JavaSecuritySpec>
	<j2se-1_4:JavaSecurityAcl rdf:about="&j2se-1_4;theJavaSecurityAclPart">
	</j2se-1_4:JavaSecurityAcl>
	<j2se-1_4:JavaSecurityInterfaces rdf:about="&j2se-1_4;theJavaSecurityInterfacesPart">
	</j2se-1_4:JavaSecurityInterfaces>
	<j2se-1_4:JavaNio rdf:about="&j2se-1_4;theJavaNioPart">
	</j2se-1_4:JavaNio>
	<j2se-1_4:JavaNioChannels rdf:about="&j2se-1_4;theJavaNioChannelsPart">
	</j2se-1_4:JavaNioChannels>
	<j2se-1_4:JavaNioChannelsSpi rdf:about="&j2se-1_4;theJavaNioChannelsSpiPart">
	</j2se-1_4:JavaNioChannelsSpi>
	<j2se-1_4:JavaNioCharset rdf:about="&j2se-1_4;theJavaNioCharsetPart">
	</j2se-1_4:JavaNioCharset>
	<j2se-1_4:JavaNioCharsetSpi rdf:about="&j2se-1_4;theJavaNioCharsetSpiPart">
	</j2se-1_4:JavaNioCharsetSpi>
	<j2se-1_4:JavaBeans rdf:about="&j2se-1_4;theJavaBeansPart">
	</j2se-1_4:JavaBeans>
	<j2se-1_4:JavaBeansBeancontext rdf:about="&j2se-1_4;theJavaBeansBeancontextPart">
	</j2se-1_4:JavaBeansBeancontext>
	<j2se-1_4:JavaAwt rdf:about="&j2se-1_4;theJavaAwtPart">
	</j2se-1_4:JavaAwt>
	<j2se-1_4:JavaAwtImage rdf:about="&j2se-1_4;theJavaAwtImagePart">
	</j2se-1_4:JavaAwtImage>
	<j2se-1_4:JavaAwtImageRenderable rdf:about="&j2se-1_4;theJavaAwtImageRenderablePart">
	</j2se-1_4:JavaAwtImageRenderable>
	<j2se-1_4:JavaAwtDatatransfer rdf:about="&j2se-1_4;theJavaAwtDatatransferPart">
	</j2se-1_4:JavaAwtDatatransfer>
	<j2se-1_4:JavaAwtDnd rdf:about="&j2se-1_4;theJavaAwtDndPart">
	</j2se-1_4:JavaAwtDnd>
	<j2se-1_4:JavaAwtEvent rdf:about="&j2se-1_4;theJavaAwtEventPart">
	</j2se-1_4:JavaAwtEvent>
	<j2se-1_4:JavaAwtIm rdf:about="&j2se-1_4;theJavaAwtImPart">
	</j2se-1_4:JavaAwtIm>
	<j2se-1_4:JavaAwtImSpi rdf:about="&j2se-1_4;theJavaAwtImSpiPart">
	</j2se-1_4:JavaAwtImSpi>
	<j2se-1_4:JavaAwtFont rdf:about="&j2se-1_4;theJavaAwtFontPart">
	</j2se-1_4:JavaAwtFont>
	<j2se-1_4:JavaAwtGeom rdf:about="&j2se-1_4;theJavaAwtGeomPart">
	</j2se-1_4:JavaAwtGeom>
	<j2se-1_4:JavaAwtColor rdf:about="&j2se-1_4;theJavaAwtColorPart">
	</j2se-1_4:JavaAwtColor>
	<j2se-1_4:JavaAwtPrint rdf:about="&j2se-1_4;theJavaAwtPrintPart">
	</j2se-1_4:JavaAwtPrint>
	<j2se-1_4:JavaText rdf:about="&j2se-1_4;theJavaTextPart">
	</j2se-1_4:JavaText>
	<j2se-1_4:JavaMath rdf:about="&j2se-1_4;theJavaMathPart">
	</j2se-1_4:JavaMath>
	<j2se-1_4:JavaApplet rdf:about="&j2se-1_4;theJavaAppletPart">
	</j2se-1_4:JavaApplet>
	<j2se-1_4:JavaRmi rdf:about="&j2se-1_4;theJavaRmiPart">
	</j2se-1_4:JavaRmi>
	<j2se-1_4:JavaRmiActivation rdf:about="&j2se-1_4;theJavaRmiActivationPart">
	</j2se-1_4:JavaRmiActivation>
	<j2se-1_4:JavaRmiServer rdf:about="&j2se-1_4;theJavaRmiServerPart">
	</j2se-1_4:JavaRmiServer>
	<j2se-1_4:JavaRmiDgc rdf:about="&j2se-1_4;theJavaRmiDgcPart">
	</j2se-1_4:JavaRmiDgc>
	<j2se-1_4:JavaRmiRegistry rdf:about="&j2se-1_4;theJavaRmiRegistryPart">
	</j2se-1_4:JavaRmiRegistry>
	<j2se-1_4:JavaSql rdf:about="&j2se-1_4;theJavaSqlPart">
	</j2se-1_4:JavaSql>
	<j2se-1_4:JavaxImageio rdf:about="&j2se-1_4;theJavaxImageioPart">
	</j2se-1_4:JavaxImageio>
	<j2se-1_4:JavaxImageioSpi rdf:about="&j2se-1_4;theJavaxImageioSpiPart">
	</j2se-1_4:JavaxImageioSpi>
	<j2se-1_4:JavaxImageioMetadata rdf:about="&j2se-1_4;theJavaxImageioMetadataPart">
	</j2se-1_4:JavaxImageioMetadata>
	<j2se-1_4:JavaxImageioStream rdf:about="&j2se-1_4;theJavaxImageioStreamPart">
	</j2se-1_4:JavaxImageioStream>
	<j2se-1_4:JavaxImageioEvent rdf:about="&j2se-1_4;theJavaxImageioEventPart">
	</j2se-1_4:JavaxImageioEvent>
	<j2se-1_4:JavaxImageioPluginsJpeg rdf:about="&j2se-1_4;theJavaxImageioPluginsJpegPart">
	</j2se-1_4:JavaxImageioPluginsJpeg>
	<j2se-1_4:JavaxAccessibility rdf:about="&j2se-1_4;theJavaxAccessibilityPart">
	</j2se-1_4:JavaxAccessibility>
	<j2se-1_4:JavaxSwing rdf:about="&j2se-1_4;theJavaxSwingPart">
	</j2se-1_4:JavaxSwing>
	<j2se-1_4:JavaxSwingPlaf rdf:about="&j2se-1_4;theJavaxSwingPlafPart">
	</j2se-1_4:JavaxSwingPlaf>
	<j2se-1_4:JavaxSwingPlafBasic rdf:about="&j2se-1_4;theJavaxSwingPlafBasicPart">
	</j2se-1_4:JavaxSwingPlafBasic>
	<j2se-1_4:JavaxSwingPlafMetal rdf:about="&j2se-1_4;theJavaxSwingPlafMetalPart">
	</j2se-1_4:JavaxSwingPlafMetal>
	<j2se-1_4:JavaxSwingPlafMulti rdf:about="&j2se-1_4;theJavaxSwingPlafMultiPart">
	</j2se-1_4:JavaxSwingPlafMulti>
	<j2se-1_4:JavaxSwingEvent rdf:about="&j2se-1_4;theJavaxSwingEventPart">
	</j2se-1_4:JavaxSwingEvent>
	<j2se-1_4:JavaxSwingBorder rdf:about="&j2se-1_4;theJavaxSwingBorderPart">
	</j2se-1_4:JavaxSwingBorder>
	<j2se-1_4:JavaxSwingText rdf:about="&j2se-1_4;theJavaxSwingTextPart">
	</j2se-1_4:JavaxSwingText>
	<j2se-1_4:JavaxSwingTextHtml rdf:about="&j2se-1_4;theJavaxSwingTextHtmlPart">
	</j2se-1_4:JavaxSwingTextHtml>
	<j2se-1_4:JavaxSwingTextHtmlParser rdf:about="&j2se-1_4;theJavaxSwingTextHtmlParserPart">
	</j2se-1_4:JavaxSwingTextHtmlParser>
	<j2se-1_4:JavaxSwingTextRtf rdf:about="&j2se-1_4;theJavaxSwingTextRtfPart">
	</j2se-1_4:JavaxSwingTextRtf>
	<j2se-1_4:JavaxSwingTable rdf:about="&j2se-1_4;theJavaxSwingTablePart">
	</j2se-1_4:JavaxSwingTable>
	<j2se-1_4:JavaxSwingUndo rdf:about="&j2se-1_4;theJavaxSwingUndoPart">
	</j2se-1_4:JavaxSwingUndo>
	<j2se-1_4:JavaxSwingTree rdf:about="&j2se-1_4;theJavaxSwingTreePart">
	</j2se-1_4:JavaxSwingTree>
	<j2se-1_4:JavaxSwingFilechooser rdf:about="&j2se-1_4;theJavaxSwingFilechooserPart">
	</j2se-1_4:JavaxSwingFilechooser>
	<j2se-1_4:JavaxSwingColorchooser rdf:about="&j2se-1_4;theJavaxSwingColorchooserPart">
	</j2se-1_4:JavaxSwingColorchooser>
	<j2se-1_4:JavaxSoundSampled rdf:about="&j2se-1_4;theJavaxSoundSampledPart">
	</j2se-1_4:JavaxSoundSampled>
	<j2se-1_4:JavaxSoundSampledSpi rdf:about="&j2se-1_4;theJavaxSoundSampledSpiPart">
	</j2se-1_4:JavaxSoundSampledSpi>
	<j2se-1_4:JavaxSoundMidi rdf:about="&j2se-1_4;theJavaxSoundMidiPart">
	</j2se-1_4:JavaxSoundMidi>
	<j2se-1_4:JavaxSoundMidiSpi rdf:about="&j2se-1_4;theJavaxSoundMidiSpiPart">
	</j2se-1_4:JavaxSoundMidiSpi>
	<j2se-1_4:JavaxPrint rdf:about="&j2se-1_4;theJavaxPrintPart">
	</j2se-1_4:JavaxPrint>
	<j2se-1_4:JavaxPrintAttribute rdf:about="&j2se-1_4;theJavaxPrintAttributePart">
	</j2se-1_4:JavaxPrintAttribute>
	<j2se-1_4:JavaxPrintAttributeStandard rdf:about="&j2se-1_4;theJavaxPrintAttributeStandardPart">
	</j2se-1_4:JavaxPrintAttributeStandard>
	<j2se-1_4:JavaxPrintEvent rdf:about="&j2se-1_4;theJavaxPrintEventPart">
	</j2se-1_4:JavaxPrintEvent>
	<j2se-1_4:JavaxSecurityAuth rdf:about="&j2se-1_4;theJavaxSecurityAuthPart">
	</j2se-1_4:JavaxSecurityAuth>
	<j2se-1_4:JavaxSecurityAuthX500 rdf:about="&j2se-1_4;theJavaxSecurityAuthX500Part">
	</j2se-1_4:JavaxSecurityAuthX500>
	<j2se-1_4:JavaxSecurityAuthCallback rdf:about="&j2se-1_4;theJavaxSecurityAuthCallbackPart">
	</j2se-1_4:JavaxSecurityAuthCallback>
	<j2se-1_4:JavaxSecurityAuthKerberos rdf:about="&j2se-1_4;theJavaxSecurityAuthKerberosPart">
	</j2se-1_4:JavaxSecurityAuthKerberos>
	<j2se-1_4:JavaxSecurityAuthLogin rdf:about="&j2se-1_4;theJavaxSecurityAuthLoginPart">
	</j2se-1_4:JavaxSecurityAuthLogin>
	<j2se-1_4:JavaxSecurityAuthSpi rdf:about="&j2se-1_4;theJavaxSecurityAuthSpiPart">
	</j2se-1_4:JavaxSecurityAuthSpi>
	<j2se-1_4:JavaxSecurityCert rdf:about="&j2se-1_4;theJavaxSecurityCertPart">
	</j2se-1_4:JavaxSecurityCert>
	<j2se-1_4:JavaxNaming rdf:about="&j2se-1_4;theJavaxNamingPart">
	</j2se-1_4:JavaxNaming>
	<j2se-1_4:JavaxNamingDirectory rdf:about="&j2se-1_4;theJavaxNamingDirectoryPart">
	</j2se-1_4:JavaxNamingDirectory>
	<j2se-1_4:JavaxNamingEvent rdf:about="&j2se-1_4;theJavaxNamingEventPart">
	</j2se-1_4:JavaxNamingEvent>
	<j2se-1_4:JavaxNamingLdap rdf:about="&j2se-1_4;theJavaxNamingLdapPart">
	</j2se-1_4:JavaxNamingLdap>
	<j2se-1_4:JavaxNamingSpi rdf:about="&j2se-1_4;theJavaxNamingSpiPart">
	</j2se-1_4:JavaxNamingSpi>
	<j2se-1_4:JavaxNet rdf:about="&j2se-1_4;theJavaxNetPart">
	</j2se-1_4:JavaxNet>
	<j2se-1_4:JavaxNetSsl rdf:about="&j2se-1_4;theJavaxNetSslPart">
	</j2se-1_4:JavaxNetSsl>
	<j2se-1_4:JavaxRmi rdf:about="&j2se-1_4;theJavaxRmiPart">
	</j2se-1_4:JavaxRmi>
	<j2se-1_4:JavaxRmiCORBA rdf:about="&j2se-1_4;theJavaxRmiCORBAPart">
	</j2se-1_4:JavaxRmiCORBA>
	<j2se-1_4:JavaxCrypto rdf:about="&j2se-1_4;theJavaxCryptoPart">
	</j2se-1_4:JavaxCrypto>
	<j2se-1_4:JavaxCryptoInterfaces rdf:about="&j2se-1_4;theJavaxCryptoInterfacesPart">
	</j2se-1_4:JavaxCryptoInterfaces>
	<j2se-1_4:JavaxCryptoSpec rdf:about="&j2se-1_4;theJavaxCryptoSpecPart">
	</j2se-1_4:JavaxCryptoSpec>
	<j2se-1_4:JavaxSql rdf:about="&j2se-1_4;theJavaxSqlPart">
	</j2se-1_4:JavaxSql>
	<j2se-1_4:JavaxTransaction rdf:about="&j2se-1_4;theJavaxTransactionPart">
	</j2se-1_4:JavaxTransaction>
	<j2se-1_4:JavaxTransactionXa rdf:about="&j2se-1_4;theJavaxTransactionXaPart">
	</j2se-1_4:JavaxTransactionXa>
	<j2se-1_4:JavaxXmlParsers rdf:about="&j2se-1_4;theJavaxXmlParsersPart">
	</j2se-1_4:JavaxXmlParsers>
	<j2se-1_4:JavaxXmlTransform rdf:about="&j2se-1_4;theJavaxXmlTransformPart">
	</j2se-1_4:JavaxXmlTransform>
	<j2se-1_4:JavaxXmlTransformDom rdf:about="&j2se-1_4;theJavaxXmlTransformDomPart">
	</j2se-1_4:JavaxXmlTransformDom>
	<j2se-1_4:JavaxXmlTransformSax rdf:about="&j2se-1_4;theJavaxXmlTransformSaxPart">
	</j2se-1_4:JavaxXmlTransformSax>
	<j2se-1_4:JavaxXmlTransformStream rdf:about="&j2se-1_4;theJavaxXmlTransformStreamPart">
	</j2se-1_4:JavaxXmlTransformStream>
	<j2se-1_4:OrgW3cDom rdf:about="&j2se-1_4;theOrgW3cDomPart">
	</j2se-1_4:OrgW3cDom>
	<j2se-1_4:OrgW3cDomCss rdf:about="&j2se-1_4;theOrgW3cDomCssPart">
	</j2se-1_4:OrgW3cDomCss>
	<j2se-1_4:OrgW3cDomStylesheets rdf:about="&j2se-1_4;theOrgW3cDomStylesheetsPart">
	</j2se-1_4:OrgW3cDomStylesheets>
	<j2se-1_4:OrgW3cDomViews rdf:about="&j2se-1_4;theOrgW3cDomViewsPart">
	</j2se-1_4:OrgW3cDomViews>
	<j2se-1_4:OrgW3cDomEvents rdf:about="&j2se-1_4;theOrgW3cDomEventsPart">
	</j2se-1_4:OrgW3cDomEvents>
	<j2se-1_4:OrgW3cDomHtml rdf:about="&j2se-1_4;theOrgW3cDomHtmlPart">
	</j2se-1_4:OrgW3cDomHtml>
	<j2se-1_4:OrgW3cDomTraversal rdf:about="&j2se-1_4;theOrgW3cDomTraversalPart">
	</j2se-1_4:OrgW3cDomTraversal>
	<j2se-1_4:OrgOmgCORBA_2_3 rdf:about="&j2se-1_4;theOrgOmgCORBA_2_3Part">
	</j2se-1_4:OrgOmgCORBA_2_3>
	<j2se-1_4:OrgOmgCORBA_2_3Portable rdf:about="&j2se-1_4;theOrgOmgCORBA_2_3PortablePart">
	</j2se-1_4:OrgOmgCORBA_2_3Portable>
	<j2se-1_4:OrgOmgCORBA rdf:about="&j2se-1_4;theOrgOmgCORBAPart">
	</j2se-1_4:OrgOmgCORBA>
	<j2se-1_4:OrgOmgCORBAPortable rdf:about="&j2se-1_4;theOrgOmgCORBAPortablePart">
	</j2se-1_4:OrgOmgCORBAPortable>
	<j2se-1_4:OrgOmgCORBADynAnyPackage rdf:about="&j2se-1_4;theOrgOmgCORBADynAnyPackagePart">
	</j2se-1_4:OrgOmgCORBADynAnyPackage>
	<j2se-1_4:OrgOmgCORBAORBPackage rdf:about="&j2se-1_4;theOrgOmgCORBAORBPackagePart">
	</j2se-1_4:OrgOmgCORBAORBPackage>
	<j2se-1_4:OrgOmgCORBATypeCodePackage rdf:about="&j2se-1_4;theOrgOmgCORBATypeCodePackagePart">
	</j2se-1_4:OrgOmgCORBATypeCodePackage>
	<j2se-1_4:OrgOmgSendingContext rdf:about="&j2se-1_4;theOrgOmgSendingContextPart">
	</j2se-1_4:OrgOmgSendingContext>
	<j2se-1_4:OrgOmgCosNaming rdf:about="&j2se-1_4;theOrgOmgCosNamingPart">
	</j2se-1_4:OrgOmgCosNaming>
	<j2se-1_4:OrgOmgCosNamingNamingContextExtPackage rdf:about="&j2se-1_4;theOrgOmgCosNamingNamingContextExtPackagePart">
	</j2se-1_4:OrgOmgCosNamingNamingContextExtPackage>
	<j2se-1_4:OrgOmgCosNamingNamingContextPackage rdf:about="&j2se-1_4;theOrgOmgCosNamingNamingContextPackagePart">
	</j2se-1_4:OrgOmgCosNamingNamingContextPackage>
	<j2se-1_4:OrgOmgPortableServer rdf:about="&j2se-1_4;theOrgOmgPortableServerPart">
	</j2se-1_4:OrgOmgPortableServer>
	<j2se-1_4:OrgOmgPortableServerCurrentPackage rdf:about="&j2se-1_4;theOrgOmgPortableServerCurrentPackagePart">
	</j2se-1_4:OrgOmgPortableServerCurrentPackage>
	<j2se-1_4:OrgOmgPortableServerPOAManagerPackage rdf:about="&j2se-1_4;theOrgOmgPortableServerPOAManagerPackagePart">
	</j2se-1_4:OrgOmgPortableServerPOAManagerPackage>
	<j2se-1_4:OrgOmgPortableServerPOAPackage rdf:about="&j2se-1_4;theOrgOmgPortableServerPOAPackagePart">
	</j2se-1_4:OrgOmgPortableServerPOAPackage>
	<j2se-1_4:OrgOmgPortableServerPortable rdf:about="&j2se-1_4;theOrgOmgPortableServerPortablePart">
	</j2se-1_4:OrgOmgPortableServerPortable>
	<j2se-1_4:OrgOmgPortableServerServantLocatorPackage rdf:about="&j2se-1_4;theOrgOmgPortableServerServantLocatorPackagePart">
	</j2se-1_4:OrgOmgPortableServerServantLocatorPackage>
	<j2se-1_4:OrgOmgDynamic rdf:about="&j2se-1_4;theOrgOmgDynamicPart">
	</j2se-1_4:OrgOmgDynamic>
	<j2se-1_4:OrgOmgDynamicAny rdf:about="&j2se-1_4;theOrgOmgDynamicAnyPart">
	</j2se-1_4:OrgOmgDynamicAny>
	<j2se-1_4:OrgOmgDynamicAnyDynAnyFactoryPackage rdf:about="&j2se-1_4;theOrgOmgDynamicAnyDynAnyFactoryPackagePart">
	</j2se-1_4:OrgOmgDynamicAnyDynAnyFactoryPackage>
	<j2se-1_4:OrgOmgDynamicAnyDynAnyPackage rdf:about="&j2se-1_4;theOrgOmgDynamicAnyDynAnyPackagePart">
	</j2se-1_4:OrgOmgDynamicAnyDynAnyPackage>
	<j2se-1_4:OrgOmgIOP rdf:about="&j2se-1_4;theOrgOmgIOPPart">
	</j2se-1_4:OrgOmgIOP>
	<j2se-1_4:OrgOmgIOPCodecFactoryPackage rdf:about="&j2se-1_4;theOrgOmgIOPCodecFactoryPackagePart">
	</j2se-1_4:OrgOmgIOPCodecFactoryPackage>
	<j2se-1_4:OrgOmgIOPCodecPackage rdf:about="&j2se-1_4;theOrgOmgIOPCodecPackagePart">
	</j2se-1_4:OrgOmgIOPCodecPackage>
	<j2se-1_4:OrgOmgMessaging rdf:about="&j2se-1_4;theOrgOmgMessagingPart">
	</j2se-1_4:OrgOmgMessaging>
	<j2se-1_4:OrgOmgPortableInterceptor rdf:about="&j2se-1_4;theOrgOmgPortableInterceptorPart">
	</j2se-1_4:OrgOmgPortableInterceptor>
	<j2se-1_4:OrgOmgPortableInterceptorORBInitInfoPackage rdf:about="&j2se-1_4;theOrgOmgPortableInterceptorORBInitInfoPackagePart">
	</j2se-1_4:OrgOmgPortableInterceptorORBInitInfoPackage>
	<j2se-1_4:OrgOmgStubJavaRmi rdf:about="&j2se-1_4;theOrgOmgStubJavaRmiPart">
	</j2se-1_4:OrgOmgStubJavaRmi>
	<j2se-1_4:OrgXmlSax rdf:about="&j2se-1_4;theOrgXmlSaxPart">
	</j2se-1_4:OrgXmlSax>
	<j2se-1_4:OrgXmlSaxHelpers rdf:about="&j2se-1_4;theOrgXmlSaxHelpersPart">
	</j2se-1_4:OrgXmlSaxHelpers>
	<j2se-1_4:OrgXmlSaxExt rdf:about="&j2se-1_4;theOrgXmlSaxExtPart">
	</j2se-1_4:OrgXmlSaxExt>
	<j2se-1_4:OrgIetfJgss rdf:about="&j2se-1_4;theOrgIetfJgssPart">
	</j2se-1_4:OrgIetfJgss>
	<owl:Class rdf:about="&j2se-1_4;JavaLangClassLibrary">
		<rdfs:subClassOf rdf:resource="&j2me-pp-1_1;JavaLangClassLibrary"/>
		<rdfs:subClassOf rdf:resource="&j2se-1_3;JavaLangClassLibrary"/>
		<rdfs:comment xml:lang="en">JavaLibrary implementing the java.lang package for J2SE 1.4</rdfs:comment>
		<rdfs:comment xml:lang="OWLManchester">platform:implementsInterface some JavaLangAPI</rdfs:comment>
	</owl:Class>
	<owl:Class rdf:about="&j2se-1_4;JavaLangReflectClassLibrary">
		<owl:equivalentClass rdf:resource="&j2me-pp-1_1;JavaLangReflectClassLibrary"/>
		<rdfs:subClassOf rdf:resource="&j2se-1_3;JavaLangReflectClassLibrary"/>
		<rdfs:comment xml:lang="en">JavaLibrary implementing the java.lang.reflect package for J2SE 1.4</rdfs:comment>
		<rdfs:comment xml:lang="OWLManchester">platform:implementsInterface some JavaLangReflectAPI</rdfs:comment>
	</owl:Class>
	<owl:Class rdf:about="&j2se-1_4;JavaLangRefClassLibrary">
		<owl:equivalentClass rdf:resource="&j2me-pp-1_1;JavaLangRefClassLibrary"/>
		<owl:equivalentClass rdf:resource="&j2se-1_3;JavaLangRefClassLibrary"/>
		<rdfs:subClassOf rdf:resource="&java;JavaClassLibrary"/>
		<rdfs:comment xml:lang="en">JavaLibrary implementing the java.lang.ref package for J2SE 1.4</rdfs:comment>
		<rdfs:comment xml:lang="OWLManchester">platform:implementsInterface some JavaLangRefAPI</rdfs:comment>
	</owl:Class>
	<owl:Class rdf:about="&j2se-1_4;JavaIoClassLibrary">
		<rdfs:subClassOf rdf:resource="&j2me-pp-1_1;JavaIoClassLibrary"/>
		<rdfs:subClassOf rdf:resource="&j2se-1_3;JavaIoClassLibrary"/>
		<rdfs:comment xml:lang="en">JavaLibrary implementing the java.io package for J2SE 1.4</rdfs:comment>
		<rdfs:comment xml:lang="OWLManchester">platform:implementsInterface some JavaIoAPI</rdfs:comment>
	</owl:Class>
	<owl:Class rdf:about="&j2se-1_4;JavaUtilClassLibrary">
		<rdfs:subClassOf rdf:resource="&j2me-pp-1_1;JavaUtilClassLibrary"/>
		<rdfs:subClassOf rdf:resource="&j2se-1_3;JavaUtilClassLibrary"/>
		<rdfs:comment xml:lang="en">JavaLibrary implementing the java.util package for J2SE 1.4</rdfs:comment>
		<rdfs:comment xml:lang="OWLManchester">platform:implementsInterface some JavaUtilAPI</rdfs:comment>
	</owl:Class>
	<owl:Class rdf:about="&j2se-1_4;JavaUtilLoggingClassLibrary">
		<rdfs:subClassOf rdf:resource="&java;JavaClassLibrary"/>
		<rdfs:comment xml:lang="en">JavaLibrary implementing the java.util.logging package for J2SE 1.4</rdfs:comment>
		<rdfs:comment xml:lang="OWLManchester">platform:implementsInterface some JavaUtilLoggingAPI</rdfs:comment>
	</owl:Class>
	<owl:Class rdf:about="&j2se-1_4;JavaUtilJarClassLibrary">
		<owl:equivalentClass rdf:resource="&j2me-pp-1_1;JavaUtilJarClassLibrary"/>
		<rdfs:subClassOf rdf:resource="&j2se-1_3;JavaUtilJarClassLibrary"/>
		<rdfs:comment xml:lang="en">JavaLibrary implementing the java.util.jar package for J2SE 1.4</rdfs:comment>
		<rdfs:comment xml:lang="OWLManchester">platform:implementsInterface some JavaUtilJarAPI</rdfs:comment>
	</owl:Class>
	<owl:Class rdf:about="&j2se-1_4;JavaUtilZipClassLibrary">
		<owl:equivalentClass rdf:resource="&j2me-pp-1_1;JavaUtilZipClassLibrary"/>
		<rdfs:subClassOf rdf:resource="&j2se-1_3;JavaUtilZipClassLibrary"/>
		<rdfs:comment xml:lang="en">JavaLibrary implementing the java.util.zip package for J2SE 1.4</rdfs:comment>
		<rdfs:comment xml:lang="OWLManchester">platform:implementsInterface some JavaUtilZipAPI</rdfs:comment>
	</owl:Class>
	<owl:Class rdf:about="&j2se-1_4;JavaUtilPrefsClassLibrary">
		<rdfs:subClassOf rdf:resource="&java;JavaClassLibrary"/>
		<rdfs:comment xml:lang="en">JavaLibrary implementing the java.util.prefs package for J2SE 1.4</rdfs:comment>
		<rdfs:comment xml:lang="OWLManchester">platform:implementsInterface some JavaUtilPrefsAPI</rdfs:comment>
	</owl:Class>
	<owl:Class rdf:about="&j2se-1_4;JavaUtilRegexClassLibrary">
		<rdfs:subClassOf rdf:resource="&java;JavaClassLibrary"/>
		<rdfs:comment xml:lang="en">JavaLibrary implementing the java.util.regex package for J2SE 1.4</rdfs:comment>
		<rdfs:comment xml:lang="OWLManchester">platform:implementsInterface some JavaUtilRegexAPI</rdfs:comment>
	</owl:Class>
	<owl:Class rdf:about="&j2se-1_4;JavaNetClassLibrary">
		<rdfs:subClassOf rdf:resource="&j2me-pp-1_1;JavaNetClassLibrary"/>
		<rdfs:subClassOf rdf:resource="&j2se-1_3;JavaNetClassLibrary"/>
		<rdfs:comment xml:lang="en">JavaLibrary implementing the java.net package for J2SE 1.4</rdfs:comment>
		<rdfs:comment xml:lang="OWLManchester">platform:implementsInterface some JavaNetAPI</rdfs:comment>
	</owl:Class>
	<owl:Class rdf:about="&j2se-1_4;JavaSecurityClassLibrary">
		<rdfs:subClassOf rdf:resource="&j2me-pp-1_1;JavaSecurityClassLibrary"/>
		<rdfs:subClassOf rdf:resource="&j2se-1_3;JavaSecurityClassLibrary"/>
		<rdfs:comment xml:lang="en">JavaLibrary implementing the java.security package for J2SE 1.4</rdfs:comment>
		<rdfs:comment xml:lang="OWLManchester">platform:implementsInterface some JavaSecurityAPI</rdfs:comment>
	</owl:Class>
	<owl:Class rdf:about="&j2se-1_4;JavaSecurityCertClassLibrary">
		<rdfs:subClassOf rdf:resource="&j2me-pp-1_1;JavaSecurityCertClassLibrary"/>
		<rdfs:subClassOf rdf:resource="&j2se-1_3;JavaSecurityCertClassLibrary"/>
		<rdfs:comment xml:lang="en">JavaLibrary implementing the java.security.cert package for J2SE 1.4</rdfs:comment>
		<rdfs:comment xml:lang="OWLManchester">platform:implementsInterface some JavaSecurityCertAPI</rdfs:comment>
	</owl:Class>
	<owl:Class rdf:about="&j2se-1_4;JavaSecuritySpecClassLibrary">
		<rdfs:subClassOf rdf:resource="&j2me-pp-1_1;JavaSecuritySpecClassLibrary"/>
		<rdfs:subClassOf rdf:resource="&j2se-1_3;JavaSecuritySpecClassLibrary"/>
		<rdfs:comment xml:lang="en">JavaLibrary implementing the java.security.spec package for J2SE 1.4</rdfs:comment>
		<rdfs:comment xml:lang="OWLManchester">platform:implementsInterface some JavaSecuritySpecAPI</rdfs:comment>
	</owl:Class>
	<owl:Class rdf:about="&j2se-1_4;JavaSecurityAclClassLibrary">
		<owl:equivalentClass rdf:resource="&j2me-pp-1_1;JavaSecurityAclClassLibrary"/>
		<rdfs:subClassOf rdf:resource="&j2se-1_3;JavaSecurityAclClassLibrary"/>
		<rdfs:comment xml:lang="en">JavaLibrary implementing the java.security.acl package for J2SE 1.4</rdfs:comment>
		<rdfs:comment xml:lang="OWLManchester">platform:implementsInterface some JavaSecurityAclAPI</rdfs:comment>
	</owl:Class>
	<owl:Class rdf:about="&j2se-1_4;JavaSecurityInterfacesClassLibrary">
		<rdfs:subClassOf rdf:resource="&j2me-pp-1_1;JavaSecurityInterfacesClassLibrary"/>
		<rdfs:subClassOf rdf:resource="&j2se-1_3;JavaSecurityInterfacesClassLibrary"/>
		<rdfs:comment xml:lang="en">JavaLibrary implementing the java.security.interfaces package for J2SE 1.4</rdfs:comment>
		<rdfs:comment xml:lang="OWLManchester">platform:implementsInterface some JavaSecurityInterfacesAPI</rdfs:comment>
	</owl:Class>
	<owl:Class rdf:about="&j2se-1_4;JavaNioClassLibrary">
		<rdfs:subClassOf rdf:resource="&java;JavaClassLibrary"/>
		<rdfs:comment xml:lang="en">JavaLibrary implementing the java.nio package for J2SE 1.4</rdfs:comment>
		<rdfs:comment xml:lang="OWLManchester">platform:implementsInterface some JavaNioAPI</rdfs:comment>
	</owl:Class>
	<owl:Class rdf:about="&j2se-1_4;JavaNioChannelsClassLibrary">
		<rdfs:subClassOf rdf:resource="&java;JavaClassLibrary"/>
		<rdfs:comment xml:lang="en">JavaLibrary implementing the java.nio.channels package for J2SE 1.4</rdfs:comment>
		<rdfs:comment xml:lang="OWLManchester">platform:implementsInterface some JavaNioChannelsAPI</rdfs:comment>
	</owl:Class>
	<owl:Class rdf:about="&j2se-1_4;JavaNioChannelsSpiClassLibrary">
		<rdfs:subClassOf rdf:resource="&java;JavaClassLibrary"/>
		<rdfs:comment xml:lang="en">JavaLibrary implementing the java.nio.channels.spi package for J2SE 1.4</rdfs:comment>
		<rdfs:comment xml:lang="OWLManchester">platform:implementsInterface some JavaNioChannelsSpiAPI</rdfs:comment>
	</owl:Class>
	<owl:Class rdf:about="&j2se-1_4;JavaNioCharsetClassLibrary">
		<rdfs:subClassOf rdf:resource="&java;JavaClassLibrary"/>
		<rdfs:comment xml:lang="en">JavaLibrary implementing the java.nio.charset package for J2SE 1.4</rdfs:comment>
		<rdfs:comment xml:lang="OWLManchester">platform:implementsInterface some JavaNioCharsetAPI</rdfs:comment>
	</owl:Class>
	<owl:Class rdf:about="&j2se-1_4;JavaNioCharsetSpiClassLibrary">
		<rdfs:subClassOf rdf:resource="&java;JavaClassLibrary"/>
		<rdfs:comment xml:lang="en">JavaLibrary implementing the java.nio.charset.spi package for J2SE 1.4</rdfs:comment>
		<rdfs:comment xml:lang="OWLManchester">platform:implementsInterface some JavaNioCharsetSpiAPI</rdfs:comment>
	</owl:Class>
	<owl:Class rdf:about="&j2se-1_4;JavaBeansClassLibrary">
		<rdfs:subClassOf rdf:resource="&j2me-pp-1_1;JavaBeansClassLibrary"/>
		<rdfs:subClassOf rdf:resource="&j2se-1_3;JavaBeansClassLibrary"/>
		<rdfs:comment xml:lang="en">JavaLibrary implementing the java.beans package for J2SE 1.4</rdfs:comment>
		<rdfs:comment xml:lang="OWLManchester">platform:implementsInterface some JavaBeansAPI</rdfs:comment>
	</owl:Class>
	<owl:Class rdf:about="&j2se-1_4;JavaBeansBeancontextClassLibrary">
		<owl:equivalentClass rdf:resource="&j2se-1_3;JavaBeansBeancontextClassLibrary"/>
		<rdfs:subClassOf rdf:resource="&java;JavaClassLibrary"/>
		<rdfs:comment xml:lang="en">JavaLibrary implementing the java.beans.beancontext package for J2SE 1.4</rdfs:comment>
		<rdfs:comment xml:lang="OWLManchester">platform:implementsInterface some JavaBeansBeancontextAPI</rdfs:comment>
	</owl:Class>
	<owl:Class rdf:about="&j2se-1_4;JavaAwtClassLibrary">
		<rdfs:subClassOf rdf:resource="&j2me-pp-1_1;JavaAwtClassLibrary"/>
		<rdfs:subClassOf rdf:resource="&j2se-1_3;JavaAwtClassLibrary"/>
		<rdfs:comment xml:lang="en">JavaLibrary implementing the java.awt package for J2SE 1.4</rdfs:comment>
		<rdfs:comment xml:lang="OWLManchester">platform:implementsInterface some JavaAwtAPI</rdfs:comment>
	</owl:Class>
	<owl:Class rdf:about="&j2se-1_4;JavaAwtImageClassLibrary">
		<rdfs:subClassOf rdf:resource="&j2me-pp-1_1;JavaAwtImageClassLibrary"/>
		<rdfs:subClassOf rdf:resource="&j2se-1_3;JavaAwtImageClassLibrary"/>
		<rdfs:comment xml:lang="en">JavaLibrary implementing the java.awt.image package for J2SE 1.4</rdfs:comment>
		<rdfs:comment xml:lang="OWLManchester">platform:implementsInterface some JavaAwtImageAPI</rdfs:comment>
	</owl:Class>
	<owl:Class rdf:about="&j2se-1_4;JavaAwtImageRenderableClassLibrary">
		<owl:equivalentClass rdf:resource="&j2se-1_3;JavaAwtImageRenderableClassLibrary"/>
		<rdfs:subClassOf rdf:resource="&java;JavaClassLibrary"/>
		<rdfs:comment xml:lang="en">JavaLibrary implementing the java.awt.image.renderable package for J2SE 1.4</rdfs:comment>
		<rdfs:comment xml:lang="OWLManchester">platform:implementsInterface some JavaAwtImageRenderableAPI</rdfs:comment>
	</owl:Class>
	<owl:Class rdf:about="&j2se-1_4;JavaAwtDatatransferClassLibrary">
		<rdfs:subClassOf rdf:resource="&j2me-pp-1_1;JavaAwtDatatransferClassLibrary"/>
		<rdfs:subClassOf rdf:resource="&j2se-1_3;JavaAwtDatatransferClassLibrary"/>
		<rdfs:comment xml:lang="en">JavaLibrary implementing the java.awt.datatransfer package for J2SE 1.4</rdfs:comment>
		<rdfs:comment xml:lang="OWLManchester">platform:implementsInterface some JavaAwtDatatransferAPI</rdfs:comment>
	</owl:Class>
	<owl:Class rdf:about="&j2se-1_4;JavaAwtDndClassLibrary">
		<rdfs:subClassOf rdf:resource="&j2se-1_3;JavaAwtDndClassLibrary"/>
		<rdfs:comment xml:lang="en">JavaLibrary implementing the java.awt.dnd package for J2SE 1.4</rdfs:comment>
		<rdfs:comment xml:lang="OWLManchester">platform:implementsInterface some JavaAwtDndAPI</rdfs:comment>
	</owl:Class>
	<owl:Class rdf:about="&j2se-1_4;JavaAwtEventClassLibrary">
		<rdfs:subClassOf rdf:resource="&j2me-pp-1_1;JavaAwtEventClassLibrary"/>
		<rdfs:subClassOf rdf:resource="&j2se-1_3;JavaAwtEventClassLibrary"/>
		<rdfs:comment xml:lang="en">JavaLibrary implementing the java.awt.event package for J2SE 1.4</rdfs:comment>
		<rdfs:comment xml:lang="OWLManchester">platform:implementsInterface some JavaAwtEventAPI</rdfs:comment>
	</owl:Class>
	<owl:Class rdf:about="&j2se-1_4;JavaAwtImClassLibrary">
		<owl:equivalentClass rdf:resource="&j2se-1_3;JavaAwtImClassLibrary"/>
		<rdfs:subClassOf rdf:resource="&j2me-pp-1_1;JavaAwtImClassLibrary"/>
		<rdfs:comment xml:lang="en">JavaLibrary implementing the java.awt.im package for J2SE 1.4</rdfs:comment>
		<rdfs:comment xml:lang="OWLManchester">platform:implementsInterface some JavaAwtImAPI</rdfs:comment>
	</owl:Class>
	<owl:Class rdf:about="&j2se-1_4;JavaAwtImSpiClassLibrary">
		<rdfs:subClassOf rdf:resource="&j2se-1_3;JavaAwtImSpiClassLibrary"/>
		<rdfs:comment xml:lang="en">JavaLibrary implementing the java.awt.im.spi package for J2SE 1.4</rdfs:comment>
		<rdfs:comment xml:lang="OWLManchester">platform:implementsInterface some JavaAwtImSpiAPI</rdfs:comment>
	</owl:Class>
	<owl:Class rdf:about="&j2se-1_4;JavaAwtFontClassLibrary">
		<rdfs:subClassOf rdf:resource="&j2me-pp-1_1;JavaAwtFontClassLibrary"/>
		<rdfs:subClassOf rdf:resource="&j2se-1_3;JavaAwtFontClassLibrary"/>
		<rdfs:comment xml:lang="en">JavaLibrary implementing the java.awt.font package for J2SE 1.4</rdfs:comment>
		<rdfs:comment xml:lang="OWLManchester">platform:implementsInterface some JavaAwtFontAPI</rdfs:comment>
	</owl:Class>
	<owl:Class rdf:about="&j2se-1_4;JavaAwtGeomClassLibrary">
		<rdfs:subClassOf rdf:resource="&j2se-1_3;JavaAwtGeomClassLibrary"/>
		<rdfs:comment xml:lang="en">JavaLibrary implementing the java.awt.geom package for J2SE 1.4</rdfs:comment>
		<rdfs:comment xml:lang="OWLManchester">platform:implementsInterface some JavaAwtGeomAPI</rdfs:comment>
	</owl:Class>
	<owl:Class rdf:about="&j2se-1_4;JavaAwtColorClassLibrary">
		<rdfs:subClassOf rdf:resource="&j2me-pp-1_1;JavaAwtColorClassLibrary"/>
		<rdfs:subClassOf rdf:resource="&j2se-1_3;JavaAwtColorClassLibrary"/>
		<rdfs:comment xml:lang="en">JavaLibrary implementing the java.awt.color package for J2SE 1.4</rdfs:comment>
		<rdfs:comment xml:lang="OWLManchester">platform:implementsInterface some JavaAwtColorAPI</rdfs:comment>
	</owl:Class>
	<owl:Class rdf:about="&j2se-1_4;JavaAwtPrintClassLibrary">
		<rdfs:subClassOf rdf:resource="&j2se-1_3;JavaAwtPrintClassLibrary"/>
		<rdfs:comment xml:lang="en">JavaLibrary implementing the java.awt.print package for J2SE 1.4</rdfs:comment>
		<rdfs:comment xml:lang="OWLManchester">platform:implementsInterface some JavaAwtPrintAPI</rdfs:comment>
	</owl:Class>
	<owl:Class rdf:about="&j2se-1_4;JavaTextClassLibrary">
		<rdfs:subClassOf rdf:resource="&j2se-1_3;JavaTextClassLibrary"/>
		<rdfs:comment xml:lang="en">JavaLibrary implementing the java.text package for J2SE 1.4</rdfs:comment>
		<rdfs:comment xml:lang="OWLManchester">platform:implementsInterface some JavaTextAPI</rdfs:comment>
	</owl:Class>
	<owl:Class rdf:about="&j2se-1_4;JavaMathClassLibrary">
		<rdfs:subClassOf rdf:resource="&j2me-pp-1_1;JavaMathClassLibrary"/>
		<rdfs:subClassOf rdf:resource="&j2se-1_3;JavaMathClassLibrary"/>
		<rdfs:comment xml:lang="en">JavaLibrary implementing the java.math package for J2SE 1.4</rdfs:comment>
		<rdfs:comment xml:lang="OWLManchester">platform:implementsInterface some JavaMathAPI</rdfs:comment>
	</owl:Class>
	<owl:Class rdf:about="&j2se-1_4;JavaAppletClassLibrary">
		<rdfs:subClassOf rdf:resource="&j2me-pp-1_1;JavaAppletClassLibrary"/>
		<rdfs:subClassOf rdf:resource="&j2se-1_3;JavaAppletClassLibrary"/>
		<rdfs:comment xml:lang="en">JavaLibrary implementing the java.applet package for J2SE 1.4</rdfs:comment>
		<rdfs:comment xml:lang="OWLManchester">platform:implementsInterface some JavaAppletAPI</rdfs:comment>
	</owl:Class>
	<owl:Class rdf:about="&j2se-1_4;JavaRmiClassLibrary">
		<rdfs:subClassOf rdf:resource="&j2me-pp-1_1;JavaRmiClassLibrary"/>
		<rdfs:subClassOf rdf:resource="&j2se-1_3;JavaRmiClassLibrary"/>
		<rdfs:comment xml:lang="en">JavaLibrary implementing the java.rmi package for J2SE 1.4</rdfs:comment>
		<rdfs:comment xml:lang="OWLManchester">platform:implementsInterface some JavaRmiAPI</rdfs:comment>
	</owl:Class>
	<owl:Class rdf:about="&j2se-1_4;JavaRmiActivationClassLibrary">
		<rdfs:subClassOf rdf:resource="&j2se-1_3;JavaRmiActivationClassLibrary"/>
		<rdfs:comment xml:lang="en">JavaLibrary implementing the java.rmi.activation package for J2SE 1.4</rdfs:comment>
		<rdfs:comment xml:lang="OWLManchester">platform:implementsInterface some JavaRmiActivationAPI</rdfs:comment>
	</owl:Class>
	<owl:Class rdf:about="&j2se-1_4;JavaRmiServerClassLibrary">
		<rdfs:subClassOf rdf:resource="&j2se-1_3;JavaRmiServerClassLibrary"/>
		<rdfs:comment xml:lang="en">JavaLibrary implementing the java.rmi.server package for J2SE 1.4</rdfs:comment>
		<rdfs:comment xml:lang="OWLManchester">platform:implementsInterface some JavaRmiServerAPI</rdfs:comment>
	</owl:Class>
	<owl:Class rdf:about="&j2se-1_4;JavaRmiDgcClassLibrary">
		<owl:equivalentClass rdf:resource="&j2se-1_3;JavaRmiDgcClassLibrary"/>
		<rdfs:subClassOf rdf:resource="&java;JavaClassLibrary"/>
		<rdfs:comment xml:lang="en">JavaLibrary implementing the java.rmi.dgc package for J2SE 1.4</rdfs:comment>
		<rdfs:comment xml:lang="OWLManchester">platform:implementsInterface some JavaRmiDgcAPI</rdfs:comment>
	</owl:Class>
	<owl:Class rdf:about="&j2se-1_4;JavaRmiRegistryClassLibrary">
		<owl:equivalentClass rdf:resource="&j2se-1_3;JavaRmiRegistryClassLibrary"/>
		<rdfs:subClassOf rdf:resource="&j2me-pp-1_1;JavaRmiRegistryClassLibrary"/>
		<rdfs:comment xml:lang="en">JavaLibrary implementing the java.rmi.registry package for J2SE 1.4</rdfs:comment>
		<rdfs:comment xml:lang="OWLManchester">platform:implementsInterface some JavaRmiRegistryAPI</rdfs:comment>
	</owl:Class>
	<owl:Class rdf:about="&j2se-1_4;JavaSqlClassLibrary">
		<rdfs:subClassOf rdf:resource="&j2se-1_3;JavaSqlClassLibrary"/>
		<rdfs:comment xml:lang="en">JavaLibrary implementing the java.sql package for J2SE 1.4</rdfs:comment>
		<rdfs:comment xml:lang="OWLManchester">platform:implementsInterface some JavaSqlAPI</rdfs:comment>
	</owl:Class>
	<owl:Class rdf:about="&j2se-1_4;JavaxImageioClassLibrary">
		<rdfs:subClassOf rdf:resource="&java;JavaClassLibrary"/>
		<rdfs:comment xml:lang="en">JavaLibrary implementing the javax.imageio package for J2SE 1.4</rdfs:comment>
		<rdfs:comment xml:lang="OWLManchester">platform:implementsInterface some JavaxImageioAPI</rdfs:comment>
	</owl:Class>
	<owl:Class rdf:about="&j2se-1_4;JavaxImageioSpiClassLibrary">
		<rdfs:subClassOf rdf:resource="&java;JavaClassLibrary"/>
		<rdfs:comment xml:lang="en">JavaLibrary implementing the javax.imageio.spi package for J2SE 1.4</rdfs:comment>
		<rdfs:comment xml:lang="OWLManchester">platform:implementsInterface some JavaxImageioSpiAPI</rdfs:comment>
	</owl:Class>
	<owl:Class rdf:about="&j2se-1_4;JavaxImageioMetadataClassLibrary">
		<rdfs:subClassOf rdf:resource="&java;JavaClassLibrary"/>
		<rdfs:comment xml:lang="en">JavaLibrary implementing the javax.imageio.metadata package for J2SE 1.4</rdfs:comment>
		<rdfs:comment xml:lang="OWLManchester">platform:implementsInterface some JavaxImageioMetadataAPI</rdfs:comment>
	</owl:Class>
	<owl:Class rdf:about="&j2se-1_4;JavaxImageioStreamClassLibrary">
		<rdfs:subClassOf rdf:resource="&java;JavaClassLibrary"/>
		<rdfs:comment xml:lang="en">JavaLibrary implementing the javax.imageio.stream package for J2SE 1.4</rdfs:comment>
		<rdfs:comment xml:lang="OWLManchester">platform:implementsInterface some JavaxImageioStreamAPI</rdfs:comment>
	</owl:Class>
	<owl:Class rdf:about="&j2se-1_4;JavaxImageioEventClassLibrary">
		<rdfs:subClassOf rdf:resource="&java;JavaClassLibrary"/>
		<rdfs:comment xml:lang="en">JavaLibrary implementing the javax.imageio.event package for J2SE 1.4</rdfs:comment>
		<rdfs:comment xml:lang="OWLManchester">platform:implementsInterface some JavaxImageioEventAPI</rdfs:comment>
	</owl:Class>
	<owl:Class rdf:about="&j2se-1_4;JavaxImageioPluginsJpegClassLibrary">
		<rdfs:subClassOf rdf:resource="&java;JavaClassLibrary"/>
		<rdfs:comment xml:lang="en">JavaLibrary implementing the javax.imageio.plugins.jpeg package for J2SE 1.4</rdfs:comment>
		<rdfs:comment xml:lang="OWLManchester">platform:implementsInterface some JavaxImageioPluginsJpegAPI</rdfs:comment>
	</owl:Class>
	<owl:Class rdf:about="&j2se-1_4;JavaxAccessibilityClassLibrary">
		<rdfs:subClassOf rdf:resource="&j2se-1_3;JavaxAccessibilityClassLibrary"/>
		<rdfs:comment xml:lang="en">JavaLibrary implementing the javax.accessibility package for J2SE 1.4</rdfs:comment>
		<rdfs:comment xml:lang="OWLManchester">platform:implementsInterface some JavaxAccessibilityAPI</rdfs:comment>
	</owl:Class>
	<owl:Class rdf:about="&j2se-1_4;JavaxSwingClassLibrary">
		<rdfs:subClassOf rdf:resource="&java;JavaClassLibrary"/>
		<rdfs:comment xml:lang="en">JavaLibrary implementing the javax.swing package for J2SE 1.4</rdfs:comment>
		<rdfs:comment xml:lang="OWLManchester">platform:implementsInterface some JavaxSwingAPI</rdfs:comment>
	</owl:Class>
	<owl:Class rdf:about="&j2se-1_4;JavaxSwingPlafClassLibrary">
		<rdfs:subClassOf rdf:resource="&j2se-1_3;JavaxSwingPlafClassLibrary"/>
		<rdfs:comment xml:lang="en">JavaLibrary implementing the javax.swing.plaf package for J2SE 1.4</rdfs:comment>
		<rdfs:comment xml:lang="OWLManchester">platform:implementsInterface some JavaxSwingPlafAPI</rdfs:comment>
	</owl:Class>
	<owl:Class rdf:about="&j2se-1_4;JavaxSwingPlafBasicClassLibrary">
		<rdfs:subClassOf rdf:resource="&j2se-1_3;JavaxSwingPlafBasicClassLibrary"/>
		<rdfs:comment xml:lang="en">JavaLibrary implementing the javax.swing.plaf.basic package for J2SE 1.4</rdfs:comment>
		<rdfs:comment xml:lang="OWLManchester">platform:implementsInterface some JavaxSwingPlafBasicAPI</rdfs:comment>
	</owl:Class>
	<owl:Class rdf:about="&j2se-1_4;JavaxSwingPlafMetalClassLibrary">
		<rdfs:subClassOf rdf:resource="&j2se-1_3;JavaxSwingPlafMetalClassLibrary"/>
		<rdfs:comment xml:lang="en">JavaLibrary implementing the javax.swing.plaf.metal package for J2SE 1.4</rdfs:comment>
		<rdfs:comment xml:lang="OWLManchester">platform:implementsInterface some JavaxSwingPlafMetalAPI</rdfs:comment>
	</owl:Class>
	<owl:Class rdf:about="&j2se-1_4;JavaxSwingPlafMultiClassLibrary">
		<rdfs:subClassOf rdf:resource="&j2se-1_3;JavaxSwingPlafMultiClassLibrary"/>
		<rdfs:comment xml:lang="en">JavaLibrary implementing the javax.swing.plaf.multi package for J2SE 1.4</rdfs:comment>
		<rdfs:comment xml:lang="OWLManchester">platform:implementsInterface some JavaxSwingPlafMultiAPI</rdfs:comment>
	</owl:Class>
	<owl:Class rdf:about="&j2se-1_4;JavaxSwingEventClassLibrary">
		<rdfs:subClassOf rdf:resource="&j2se-1_3;JavaxSwingEventClassLibrary"/>
		<rdfs:comment xml:lang="en">JavaLibrary implementing the javax.swing.event package for J2SE 1.4</rdfs:comment>
		<rdfs:comment xml:lang="OWLManchester">platform:implementsInterface some JavaxSwingEventAPI</rdfs:comment>
	</owl:Class>
	<owl:Class rdf:about="&j2se-1_4;JavaxSwingBorderClassLibrary">
		<owl:equivalentClass rdf:resource="&j2se-1_3;JavaxSwingBorderClassLibrary"/>
		<rdfs:subClassOf rdf:resource="&java;JavaClassLibrary"/>
		<rdfs:comment xml:lang="en">JavaLibrary implementing the javax.swing.border package for J2SE 1.4</rdfs:comment>
		<rdfs:comment xml:lang="OWLManchester">platform:implementsInterface some JavaxSwingBorderAPI</rdfs:comment>
	</owl:Class>
	<owl:Class rdf:about="&j2se-1_4;JavaxSwingTextClassLibrary">
		<rdfs:subClassOf rdf:resource="&j2se-1_3;JavaxSwingTextClassLibrary"/>
		<rdfs:comment xml:lang="en">JavaLibrary implementing the javax.swing.text package for J2SE 1.4</rdfs:comment>
		<rdfs:comment xml:lang="OWLManchester">platform:implementsInterface some JavaxSwingTextAPI</rdfs:comment>
	</owl:Class>
	<owl:Class rdf:about="&j2se-1_4;JavaxSwingTextHtmlClassLibrary">
		<rdfs:subClassOf rdf:resource="&j2se-1_3;JavaxSwingTextHtmlClassLibrary"/>
		<rdfs:comment xml:lang="en">JavaLibrary implementing the javax.swing.text.html package for J2SE 1.4</rdfs:comment>
		<rdfs:comment xml:lang="OWLManchester">platform:implementsInterface some JavaxSwingTextHtmlAPI</rdfs:comment>
	</owl:Class>
	<owl:Class rdf:about="&j2se-1_4;JavaxSwingTextHtmlParserClassLibrary">
		<owl:equivalentClass rdf:resource="&j2se-1_3;JavaxSwingTextHtmlParserClassLibrary"/>
		<rdfs:subClassOf rdf:resource="&java;JavaClassLibrary"/>
		<rdfs:comment xml:lang="en">JavaLibrary implementing the javax.swing.text.html.parser package for J2SE 1.4</rdfs:comment>
		<rdfs:comment xml:lang="OWLManchester">platform:implementsInterface some JavaxSwingTextHtmlParserAPI</rdfs:comment>
	</owl:Class>
	<owl:Class rdf:about="&j2se-1_4;JavaxSwingTextRtfClassLibrary">
		<owl:equivalentClass rdf:resource="&j2se-1_3;JavaxSwingTextRtfClassLibrary"/>
		<rdfs:subClassOf rdf:resource="&java;JavaClassLibrary"/>
		<rdfs:comment xml:lang="en">JavaLibrary implementing the javax.swing.text.rtf package for J2SE 1.4</rdfs:comment>
		<rdfs:comment xml:lang="OWLManchester">platform:implementsInterface some JavaxSwingTextRtfAPI</rdfs:comment>
	</owl:Class>
	<owl:Class rdf:about="&j2se-1_4;JavaxSwingTableClassLibrary">
		<rdfs:subClassOf rdf:resource="&j2se-1_3;JavaxSwingTableClassLibrary"/>
		<rdfs:comment xml:lang="en">JavaLibrary implementing the javax.swing.table package for J2SE 1.4</rdfs:comment>
		<rdfs:comment xml:lang="OWLManchester">platform:implementsInterface some JavaxSwingTableAPI</rdfs:comment>
	</owl:Class>
	<owl:Class rdf:about="&j2se-1_4;JavaxSwingUndoClassLibrary">
		<rdfs:subClassOf rdf:resource="&j2se-1_3;JavaxSwingUndoClassLibrary"/>
		<rdfs:comment xml:lang="en">JavaLibrary implementing the javax.swing.undo package for J2SE 1.4</rdfs:comment>
		<rdfs:comment xml:lang="OWLManchester">platform:implementsInterface some JavaxSwingUndoAPI</rdfs:comment>
	</owl:Class>
	<owl:Class rdf:about="&j2se-1_4;JavaxSwingTreeClassLibrary">
		<rdfs:subClassOf rdf:resource="&j2se-1_3;JavaxSwingTreeClassLibrary"/>
		<rdfs:comment xml:lang="en">JavaLibrary implementing the javax.swing.tree package for J2SE 1.4</rdfs:comment>
		<rdfs:comment xml:lang="OWLManchester">platform:implementsInterface some JavaxSwingTreeAPI</rdfs:comment>
	</owl:Class>
	<owl:Class rdf:about="&j2se-1_4;JavaxSwingFilechooserClassLibrary">
		<rdfs:subClassOf rdf:resource="&j2se-1_3;JavaxSwingFilechooserClassLibrary"/>
		<rdfs:comment xml:lang="en">JavaLibrary implementing the javax.swing.filechooser package for J2SE 1.4</rdfs:comment>
		<rdfs:comment xml:lang="OWLManchester">platform:implementsInterface some JavaxSwingFilechooserAPI</rdfs:comment>
	</owl:Class>
	<owl:Class rdf:about="&j2se-1_4;JavaxSwingColorchooserClassLibrary">
		<rdfs:subClassOf rdf:resource="&j2se-1_3;JavaxSwingColorchooserClassLibrary"/>
		<rdfs:comment xml:lang="en">JavaLibrary implementing the javax.swing.colorchooser package for J2SE 1.4</rdfs:comment>
		<rdfs:comment xml:lang="OWLManchester">platform:implementsInterface some JavaxSwingColorchooserAPI</rdfs:comment>
	</owl:Class>
	<owl:Class rdf:about="&j2se-1_4;JavaxSoundSampledClassLibrary">
		<rdfs:subClassOf rdf:resource="&j2se-1_3;JavaxSoundSampledClassLibrary"/>
		<rdfs:comment xml:lang="en">JavaLibrary implementing the javax.sound.sampled package for J2SE 1.4</rdfs:comment>
		<rdfs:comment xml:lang="OWLManchester">platform:implementsInterface some JavaxSoundSampledAPI</rdfs:comment>
	</owl:Class>
	<owl:Class rdf:about="&j2se-1_4;JavaxSoundSampledSpiClassLibrary">
		<owl:equivalentClass rdf:resource="&j2se-1_3;JavaxSoundSampledSpiClassLibrary"/>
		<rdfs:subClassOf rdf:resource="&java;JavaClassLibrary"/>
		<rdfs:comment xml:lang="en">JavaLibrary implementing the javax.sound.sampled.spi package for J2SE 1.4</rdfs:comment>
		<rdfs:comment xml:lang="OWLManchester">platform:implementsInterface some JavaxSoundSampledSpiAPI</rdfs:comment>
	</owl:Class>
	<owl:Class rdf:about="&j2se-1_4;JavaxSoundMidiClassLibrary">
		<rdfs:subClassOf rdf:resource="&j2se-1_3;JavaxSoundMidiClassLibrary"/>
		<rdfs:comment xml:lang="en">JavaLibrary implementing the javax.sound.midi package for J2SE 1.4</rdfs:comment>
		<rdfs:comment xml:lang="OWLManchester">platform:implementsInterface some JavaxSoundMidiAPI</rdfs:comment>
	</owl:Class>
	<owl:Class rdf:about="&j2se-1_4;JavaxSoundMidiSpiClassLibrary">
		<owl:equivalentClass rdf:resource="&j2se-1_3;JavaxSoundMidiSpiClassLibrary"/>
		<rdfs:subClassOf rdf:resource="&java;JavaClassLibrary"/>
		<rdfs:comment xml:lang="en">JavaLibrary implementing the javax.sound.midi.spi package for J2SE 1.4</rdfs:comment>
		<rdfs:comment xml:lang="OWLManchester">platform:implementsInterface some JavaxSoundMidiSpiAPI</rdfs:comment>
	</owl:Class>
	<owl:Class rdf:about="&j2se-1_4;JavaxPrintClassLibrary">
		<rdfs:subClassOf rdf:resource="&java;JavaClassLibrary"/>
		<rdfs:comment xml:lang="en">JavaLibrary implementing the javax.print package for J2SE 1.4</rdfs:comment>
		<rdfs:comment xml:lang="OWLManchester">platform:implementsInterface some JavaxPrintAPI</rdfs:comment>
	</owl:Class>
	<owl:Class rdf:about="&j2se-1_4;JavaxPrintAttributeClassLibrary">
		<rdfs:subClassOf rdf:resource="&java;JavaClassLibrary"/>
		<rdfs:comment xml:lang="en">JavaLibrary implementing the javax.print.attribute package for J2SE 1.4</rdfs:comment>
		<rdfs:comment xml:lang="OWLManchester">platform:implementsInterface some JavaxPrintAttributeAPI</rdfs:comment>
	</owl:Class>
	<owl:Class rdf:about="&j2se-1_4;JavaxPrintAttributeStandardClassLibrary">
		<rdfs:subClassOf rdf:resource="&java;JavaClassLibrary"/>
		<rdfs:comment xml:lang="en">JavaLibrary implementing the javax.print.attribute.standard package for J2SE 1.4</rdfs:comment>
		<rdfs:comment xml:lang="OWLManchester">platform:implementsInterface some JavaxPrintAttributeStandardAPI</rdfs:comment>
	</owl:Class>
	<owl:Class rdf:about="&j2se-1_4;JavaxPrintEventClassLibrary">
		<rdfs:subClassOf rdf:resource="&java;JavaClassLibrary"/>
		<rdfs:comment xml:lang="en">JavaLibrary implementing the javax.print.event package for J2SE 1.4</rdfs:comment>
		<rdfs:comment xml:lang="OWLManchester">platform:implementsInterface some JavaxPrintEventAPI</rdfs:comment>
	</owl:Class>
	<owl:Class rdf:about="&j2se-1_4;JavaxSecurityAuthClassLibrary">
		<rdfs:subClassOf rdf:resource="&java;JavaClassLibrary"/>
		<rdfs:comment xml:lang="en">JavaLibrary implementing the javax.security.auth package for J2SE 1.4</rdfs:comment>
		<rdfs:comment xml:lang="OWLManchester">platform:implementsInterface some JavaxSecurityAuthAPI</rdfs:comment>
	</owl:Class>
	<owl:Class rdf:about="&j2se-1_4;JavaxSecurityAuthX500ClassLibrary">
		<rdfs:subClassOf rdf:resource="&j2me-pp-1_1;JavaxSecurityAuthX500ClassLibrary"/>
		<rdfs:comment xml:lang="en">JavaLibrary implementing the javax.security.auth.x500 package for J2SE 1.4</rdfs:comment>
		<rdfs:comment xml:lang="OWLManchester">platform:implementsInterface some JavaxSecurityAuthX500API</rdfs:comment>
	</owl:Class>
	<owl:Class rdf:about="&j2se-1_4;JavaxSecurityAuthCallbackClassLibrary">
		<rdfs:subClassOf rdf:resource="&java;JavaClassLibrary"/>
		<rdfs:comment xml:lang="en">JavaLibrary implementing the javax.security.auth.callback package for J2SE 1.4</rdfs:comment>
		<rdfs:comment xml:lang="OWLManchester">platform:implementsInterface some JavaxSecurityAuthCallbackAPI</rdfs:comment>
	</owl:Class>
	<owl:Class rdf:about="&j2se-1_4;JavaxSecurityAuthKerberosClassLibrary">
		<rdfs:subClassOf rdf:resource="&java;JavaClassLibrary"/>
		<rdfs:comment xml:lang="en">JavaLibrary implementing the javax.security.auth.kerberos package for J2SE 1.4</rdfs:comment>
		<rdfs:comment xml:lang="OWLManchester">platform:implementsInterface some JavaxSecurityAuthKerberosAPI</rdfs:comment>
	</owl:Class>
	<owl:Class rdf:about="&j2se-1_4;JavaxSecurityAuthLoginClassLibrary">
		<rdfs:subClassOf rdf:resource="&java;JavaClassLibrary"/>
		<rdfs:comment xml:lang="en">JavaLibrary implementing the javax.security.auth.login package for J2SE 1.4</rdfs:comment>
		<rdfs:comment xml:lang="OWLManchester">platform:implementsInterface some JavaxSecurityAuthLoginAPI</rdfs:comment>
	</owl:Class>
	<owl:Class rdf:about="&j2se-1_4;JavaxSecurityAuthSpiClassLibrary">
		<rdfs:subClassOf rdf:resource="&java;JavaClassLibrary"/>
		<rdfs:comment xml:lang="en">JavaLibrary implementing the javax.security.auth.spi package for J2SE 1.4</rdfs:comment>
		<rdfs:comment xml:lang="OWLManchester">platform:implementsInterface some JavaxSecurityAuthSpiAPI</rdfs:comment>
	</owl:Class>
	<owl:Class rdf:about="&j2se-1_4;JavaxSecurityCertClassLibrary">
		<rdfs:subClassOf rdf:resource="&java;JavaClassLibrary"/>
		<rdfs:comment xml:lang="en">JavaLibrary implementing the javax.security.cert package for J2SE 1.4</rdfs:comment>
		<rdfs:comment xml:lang="OWLManchester">platform:implementsInterface some JavaxSecurityCertAPI</rdfs:comment>
	</owl:Class>
	<owl:Class rdf:about="&j2se-1_4;JavaxNamingClassLibrary">
		<rdfs:subClassOf rdf:resource="&j2se-1_3;JavaxNamingClassLibrary"/>
		<rdfs:comment xml:lang="en">JavaLibrary implementing the javax.naming package for J2SE 1.4</rdfs:comment>
		<rdfs:comment xml:lang="OWLManchester">platform:implementsInterface some JavaxNamingAPI</rdfs:comment>
	</owl:Class>
	<owl:Class rdf:about="&j2se-1_4;JavaxNamingDirectoryClassLibrary">
		<rdfs:subClassOf rdf:resource="&j2se-1_3;JavaxNamingDirectoryClassLibrary"/>
		<rdfs:comment xml:lang="en">JavaLibrary implementing the javax.naming.directory package for J2SE 1.4</rdfs:comment>
		<rdfs:comment xml:lang="OWLManchester">platform:implementsInterface some JavaxNamingDirectoryAPI</rdfs:comment>
	</owl:Class>
	<owl:Class rdf:about="&j2se-1_4;JavaxNamingEventClassLibrary">
		<owl:equivalentClass rdf:resource="&j2se-1_3;JavaxNamingEventClassLibrary"/>
		<rdfs:subClassOf rdf:resource="&java;JavaClassLibrary"/>
		<rdfs:comment xml:lang="en">JavaLibrary implementing the javax.naming.event package for J2SE 1.4</rdfs:comment>
		<rdfs:comment xml:lang="OWLManchester">platform:implementsInterface some JavaxNamingEventAPI</rdfs:comment>
	</owl:Class>
	<owl:Class rdf:about="&j2se-1_4;JavaxNamingLdapClassLibrary">
		<rdfs:subClassOf rdf:resource="&j2se-1_3;JavaxNamingLdapClassLibrary"/>
		<rdfs:comment xml:lang="en">JavaLibrary implementing the javax.naming.ldap package for J2SE 1.4</rdfs:comment>
		<rdfs:comment xml:lang="OWLManchester">platform:implementsInterface some JavaxNamingLdapAPI</rdfs:comment>
	</owl:Class>
	<owl:Class rdf:about="&j2se-1_4;JavaxNamingSpiClassLibrary">
		<owl:equivalentClass rdf:resource="&j2se-1_3;JavaxNamingSpiClassLibrary"/>
		<rdfs:subClassOf rdf:resource="&java;JavaClassLibrary"/>
		<rdfs:comment xml:lang="en">JavaLibrary implementing the javax.naming.spi package for J2SE 1.4</rdfs:comment>
		<rdfs:comment xml:lang="OWLManchester">platform:implementsInterface some JavaxNamingSpiAPI</rdfs:comment>
	</owl:Class>
	<owl:Class rdf:about="&j2se-1_4;JavaxNetClassLibrary">
		<rdfs:subClassOf rdf:resource="&java;JavaClassLibrary"/>
		<rdfs:comment xml:lang="en">JavaLibrary implementing the javax.net package for J2SE 1.4</rdfs:comment>
		<rdfs:comment xml:lang="OWLManchester">platform:implementsInterface some JavaxNetAPI</rdfs:comment>
	</owl:Class>
	<owl:Class rdf:about="&j2se-1_4;JavaxNetSslClassLibrary">
		<rdfs:subClassOf rdf:resource="&java;JavaClassLibrary"/>
		<rdfs:comment xml:lang="en">JavaLibrary implementing the javax.net.ssl package for J2SE 1.4</rdfs:comment>
		<rdfs:comment xml:lang="OWLManchester">platform:implementsInterface some JavaxNetSslAPI</rdfs:comment>
	</owl:Class>
	<owl:Class rdf:about="&j2se-1_4;JavaxRmiClassLibrary">
		<owl:equivalentClass rdf:resource="&j2se-1_3;JavaxRmiClassLibrary"/>
		<rdfs:subClassOf rdf:resource="&java;JavaClassLibrary"/>
		<rdfs:comment xml:lang="en">JavaLibrary implementing the javax.rmi package for J2SE 1.4</rdfs:comment>
		<rdfs:comment xml:lang="OWLManchester">platform:implementsInterface some JavaxRmiAPI</rdfs:comment>
	</owl:Class>
	<owl:Class rdf:about="&j2se-1_4;JavaxRmiCORBAClassLibrary">
		<owl:equivalentClass rdf:resource="&j2se-1_3;JavaxRmiCORBAClassLibrary"/>
		<rdfs:subClassOf rdf:resource="&java;JavaClassLibrary"/>
		<rdfs:comment xml:lang="en">JavaLibrary implementing the javax.rmi.CORBA package for J2SE 1.4</rdfs:comment>
		<rdfs:comment xml:lang="OWLManchester">platform:implementsInterface some JavaxRmiCORBAAPI</rdfs:comment>
	</owl:Class>
	<owl:Class rdf:about="&j2se-1_4;JavaxCryptoClassLibrary">
		<rdfs:subClassOf rdf:resource="&java;JavaClassLibrary"/>
		<rdfs:comment xml:lang="en">JavaLibrary implementing the javax.crypto package for J2SE 1.4</rdfs:comment>
		<rdfs:comment xml:lang="OWLManchester">platform:implementsInterface some JavaxCryptoAPI</rdfs:comment>
	</owl:Class>
	<owl:Class rdf:about="&j2se-1_4;JavaxCryptoInterfacesClassLibrary">
		<rdfs:subClassOf rdf:resource="&java;JavaClassLibrary"/>
		<rdfs:comment xml:lang="en">JavaLibrary implementing the javax.crypto.interfaces package for J2SE 1.4</rdfs:comment>
		<rdfs:comment xml:lang="OWLManchester">platform:implementsInterface some JavaxCryptoInterfacesAPI</rdfs:comment>
	</owl:Class>
	<owl:Class rdf:about="&j2se-1_4;JavaxCryptoSpecClassLibrary">
		<rdfs:subClassOf rdf:resource="&java;JavaClassLibrary"/>
		<rdfs:comment xml:lang="en">JavaLibrary implementing the javax.crypto.spec package for J2SE 1.4</rdfs:comment>
		<rdfs:comment xml:lang="OWLManchester">platform:implementsInterface some JavaxCryptoSpecAPI</rdfs:comment>
	</owl:Class>
	<owl:Class rdf:about="&j2se-1_4;JavaxSqlClassLibrary">
		<rdfs:subClassOf rdf:resource="&java;JavaClassLibrary"/>
		<rdfs:comment xml:lang="en">JavaLibrary implementing the javax.sql package for J2SE 1.4</rdfs:comment>
		<rdfs:comment xml:lang="OWLManchester">platform:implementsInterface some JavaxSqlAPI</rdfs:comment>
	</owl:Class>
	<owl:Class rdf:about="&j2se-1_4;JavaxTransactionClassLibrary">
		<rdfs:subClassOf rdf:resource="&j2se-1_3;JavaxTransactionClassLibrary"/>
		<rdfs:comment xml:lang="en">JavaLibrary implementing the javax.transaction package for J2SE 1.4</rdfs:comment>
		<rdfs:comment xml:lang="OWLManchester">platform:implementsInterface some JavaxTransactionAPI</rdfs:comment>
	</owl:Class>
	<owl:Class rdf:about="&j2se-1_4;JavaxTransactionXaClassLibrary">
		<rdfs:subClassOf rdf:resource="&java;JavaClassLibrary"/>
		<rdfs:comment xml:lang="en">JavaLibrary implementing the javax.transaction.xa package for J2SE 1.4</rdfs:comment>
		<rdfs:comment xml:lang="OWLManchester">platform:implementsInterface some JavaxTransactionXaAPI</rdfs:comment>
	</owl:Class>
	<owl:Class rdf:about="&j2se-1_4;JavaxXmlParsersClassLibrary">
		<rdfs:subClassOf rdf:resource="&java;JavaClassLibrary"/>
		<rdfs:comment xml:lang="en">JavaLibrary implementing the javax.xml.parsers package for J2SE 1.4</rdfs:comment>
		<rdfs:comment xml:lang="OWLManchester">platform:implementsInterface some JavaxXmlParsersAPI</rdfs:comment>
	</owl:Class>
	<owl:Class rdf:about="&j2se-1_4;JavaxXmlTransformClassLibrary">
		<rdfs:subClassOf rdf:resource="&java;JavaClassLibrary"/>
		<rdfs:comment xml:lang="en">JavaLibrary implementing the javax.xml.transform package for J2SE 1.4</rdfs:comment>
		<rdfs:comment xml:lang="OWLManchester">platform:implementsInterface some JavaxXmlTransformAPI</rdfs:comment>
	</owl:Class>
	<owl:Class rdf:about="&j2se-1_4;JavaxXmlTransformDomClassLibrary">
		<rdfs:subClassOf rdf:resource="&java;JavaClassLibrary"/>
		<rdfs:comment xml:lang="en">JavaLibrary implementing the javax.xml.transform.dom package for J2SE 1.4</rdfs:comment>
		<rdfs:comment xml:lang="OWLManchester">platform:implementsInterface some JavaxXmlTransformDomAPI</rdfs:comment>
	</owl:Class>
	<owl:Class rdf:about="&j2se-1_4;JavaxXmlTransformSaxClassLibrary">
		<rdfs:subClassOf rdf:resource="&java;JavaClassLibrary"/>
		<rdfs:comment xml:lang="en">JavaLibrary implementing the javax.xml.transform.sax package for J2SE 1.4</rdfs:comment>
		<rdfs:comment xml:lang="OWLManchester">platform:implementsInterface some JavaxXmlTransformSaxAPI</rdfs:comment>
	</owl:Class>
	<owl:Class rdf:about="&j2se-1_4;JavaxXmlTransformStreamClassLibrary">
		<rdfs:subClassOf rdf:resource="&java;JavaClassLibrary"/>
		<rdfs:comment xml:lang="en">JavaLibrary implementing the javax.xml.transform.stream package for J2SE 1.4</rdfs:comment>
		<rdfs:comment xml:lang="OWLManchester">platform:implementsInterface some JavaxXmlTransformStreamAPI</rdfs:comment>
	</owl:Class>
	<owl:Class rdf:about="&j2se-1_4;OrgW3cDomClassLibrary">
		<rdfs:subClassOf rdf:resource="&java;JavaClassLibrary"/>
		<rdfs:comment xml:lang="en">JavaLibrary implementing the org.w3c.dom package for J2SE 1.4</rdfs:comment>
		<rdfs:comment xml:lang="OWLManchester">platform:implementsInterface some OrgW3cDomAPI</rdfs:comment>
	</owl:Class>
	<owl:Class rdf:about="&j2se-1_4;OrgW3cDomCssClassLibrary">
		<rdfs:subClassOf rdf:resource="&java;JavaClassLibrary"/>
		<rdfs:comment xml:lang="en">JavaLibrary implementing the org.w3c.dom.css package for J2SE 1.4</rdfs:comment>
		<rdfs:comment xml:lang="OWLManchester">platform:implementsInterface some OrgW3cDomCssAPI</rdfs:comment>
	</owl:Class>
	<owl:Class rdf:about="&j2se-1_4;OrgW3cDomStylesheetsClassLibrary">
		<rdfs:subClassOf rdf:resource="&java;JavaClassLibrary"/>
		<rdfs:comment xml:lang="en">JavaLibrary implementing the org.w3c.dom.stylesheets package for J2SE 1.4</rdfs:comment>
		<rdfs:comment xml:lang="OWLManchester">platform:implementsInterface some OrgW3cDomStylesheetsAPI</rdfs:comment>
	</owl:Class>
	<owl:Class rdf:about="&j2se-1_4;OrgW3cDomViewsClassLibrary">
		<rdfs:subClassOf rdf:resource="&java;JavaClassLibrary"/>
		<rdfs:comment xml:lang="en">JavaLibrary implementing the org.w3c.dom.views package for J2SE 1.4</rdfs:comment>
		<rdfs:comment xml:lang="OWLManchester">platform:implementsInterface some OrgW3cDomViewsAPI</rdfs:comment>
	</owl:Class>
	<owl:Class rdf:about="&j2se-1_4;OrgW3cDomEventsClassLibrary">
		<rdfs:subClassOf rdf:resource="&java;JavaClassLibrary"/>
		<rdfs:comment xml:lang="en">JavaLibrary implementing the org.w3c.dom.events package for J2SE 1.4</rdfs:comment>
		<rdfs:comment xml:lang="OWLManchester">platform:implementsInterface some OrgW3cDomEventsAPI</rdfs:comment>
	</owl:Class>
	<owl:Class rdf:about="&j2se-1_4;OrgW3cDomHtmlClassLibrary">
		<rdfs:subClassOf rdf:resource="&java;JavaClassLibrary"/>
		<rdfs:comment xml:lang="en">JavaLibrary implementing the org.w3c.dom.html package for J2SE 1.4</rdfs:comment>
		<rdfs:comment xml:lang="OWLManchester">platform:implementsInterface some OrgW3cDomHtmlAPI</rdfs:comment>
	</owl:Class>
	<owl:Class rdf:about="&j2se-1_4;OrgW3cDomTraversalClassLibrary">
		<rdfs:subClassOf rdf:resource="&java;JavaClassLibrary"/>
		<rdfs:comment xml:lang="en">JavaLibrary implementing the org.w3c.dom.traversal package for J2SE 1.4</rdfs:comment>
		<rdfs:comment xml:lang="OWLManchester">platform:implementsInterface some OrgW3cDomTraversalAPI</rdfs:comment>
	</owl:Class>
	<owl:Class rdf:about="&j2se-1_4;OrgOmgCORBA_2_3ClassLibrary">
		<owl:equivalentClass rdf:resource="&j2se-1_3;OrgOmgCORBA_2_3ClassLibrary"/>
		<rdfs:subClassOf rdf:resource="&java;JavaClassLibrary"/>
		<rdfs:comment xml:lang="en">JavaLibrary implementing the org.omg.CORBA_2_3 package for J2SE 1.4</rdfs:comment>
		<rdfs:comment xml:lang="OWLManchester">platform:implementsInterface some OrgOmgCORBA_2_3API</rdfs:comment>
	</owl:Class>
	<owl:Class rdf:about="&j2se-1_4;OrgOmgCORBA_2_3PortableClassLibrary">
		<rdfs:subClassOf rdf:resource="&java;JavaClassLibrary"/>
		<rdfs:comment xml:lang="en">JavaLibrary implementing the org.omg.CORBA_2_3.portable package for J2SE 1.4</rdfs:comment>
		<rdfs:comment xml:lang="OWLManchester">platform:implementsInterface some OrgOmgCORBA_2_3PortableAPI</rdfs:comment>
	</owl:Class>
	<owl:Class rdf:about="&j2se-1_4;OrgOmgCORBAClassLibrary">
		<rdfs:subClassOf rdf:resource="&java;JavaClassLibrary"/>
		<rdfs:comment xml:lang="en">JavaLibrary implementing the org.omg.CORBA package for J2SE 1.4</rdfs:comment>
		<rdfs:comment xml:lang="OWLManchester">platform:implementsInterface some OrgOmgCORBAAPI</rdfs:comment>
	</owl:Class>
	<owl:Class rdf:about="&j2se-1_4;OrgOmgCORBAPortableClassLibrary">
		<rdfs:subClassOf rdf:resource="&java;JavaClassLibrary"/>
		<rdfs:comment xml:lang="en">JavaLibrary implementing the org.omg.CORBA.portable package for J2SE 1.4</rdfs:comment>
		<rdfs:comment xml:lang="OWLManchester">platform:implementsInterface some OrgOmgCORBAPortableAPI</rdfs:comment>
	</owl:Class>
	<owl:Class rdf:about="&j2se-1_4;OrgOmgCORBADynAnyPackageClassLibrary">
		<rdfs:subClassOf rdf:resource="&j2se-1_3;OrgOmgCORBADynAnyPackageClassLibrary"/>
		<rdfs:comment xml:lang="en">JavaLibrary implementing the org.omg.CORBA.DynAnyPackage package for J2SE 1.4</rdfs:comment>
		<rdfs:comment xml:lang="OWLManchester">platform:implementsInterface some OrgOmgCORBADynAnyPackageAPI</rdfs:comment>
	</owl:Class>
	<owl:Class rdf:about="&j2se-1_4;OrgOmgCORBAORBPackageClassLibrary">
		<rdfs:subClassOf rdf:resource="&j2se-1_3;OrgOmgCORBAORBPackageClassLibrary"/>
		<rdfs:comment xml:lang="en">JavaLibrary implementing the org.omg.CORBA.ORBPackage package for J2SE 1.4</rdfs:comment>
		<rdfs:comment xml:lang="OWLManchester">platform:implementsInterface some OrgOmgCORBAORBPackageAPI</rdfs:comment>
	</owl:Class>
	<owl:Class rdf:about="&j2se-1_4;OrgOmgCORBATypeCodePackageClassLibrary">
		<rdfs:subClassOf rdf:resource="&j2se-1_3;OrgOmgCORBATypeCodePackageClassLibrary"/>
		<rdfs:comment xml:lang="en">JavaLibrary implementing the org.omg.CORBA.TypeCodePackage package for J2SE 1.4</rdfs:comment>
		<rdfs:comment xml:lang="OWLManchester">platform:implementsInterface some OrgOmgCORBATypeCodePackageAPI</rdfs:comment>
	</owl:Class>
	<owl:Class rdf:about="&j2se-1_4;OrgOmgSendingContextClassLibrary">
		<owl:equivalentClass rdf:resource="&j2se-1_3;OrgOmgSendingContextClassLibrary"/>
		<rdfs:subClassOf rdf:resource="&java;JavaClassLibrary"/>
		<rdfs:comment xml:lang="en">JavaLibrary implementing the org.omg.SendingContext package for J2SE 1.4</rdfs:comment>
		<rdfs:comment xml:lang="OWLManchester">platform:implementsInterface some OrgOmgSendingContextAPI</rdfs:comment>
	</owl:Class>
	<owl:Class rdf:about="&j2se-1_4;OrgOmgCosNamingClassLibrary">
		<rdfs:subClassOf rdf:resource="&java;JavaClassLibrary"/>
		<rdfs:comment xml:lang="en">JavaLibrary implementing the org.omg.CosNaming package for J2SE 1.4</rdfs:comment>
		<rdfs:comment xml:lang="OWLManchester">platform:implementsInterface some OrgOmgCosNamingAPI</rdfs:comment>
	</owl:Class>
	<owl:Class rdf:about="&j2se-1_4;OrgOmgCosNamingNamingContextExtPackageClassLibrary">
		<rdfs:subClassOf rdf:resource="&java;JavaClassLibrary"/>
		<rdfs:comment xml:lang="en">JavaLibrary implementing the org.omg.CosNaming.NamingContextExtPackage package for J2SE 1.4</rdfs:comment>
		<rdfs:comment xml:lang="OWLManchester">platform:implementsInterface some OrgOmgCosNamingNamingContextExtPackageAPI</rdfs:comment>
	</owl:Class>
	<owl:Class rdf:about="&j2se-1_4;OrgOmgCosNamingNamingContextPackageClassLibrary">
		<rdfs:subClassOf rdf:resource="&java;JavaClassLibrary"/>
		<rdfs:comment xml:lang="en">JavaLibrary implementing the org.omg.CosNaming.NamingContextPackage package for J2SE 1.4</rdfs:comment>
		<rdfs:comment xml:lang="OWLManchester">platform:implementsInterface some OrgOmgCosNamingNamingContextPackageAPI</rdfs:comment>
	</owl:Class>
	<owl:Class rdf:about="&j2se-1_4;OrgOmgPortableServerClassLibrary">
		<rdfs:subClassOf rdf:resource="&java;JavaClassLibrary"/>
		<rdfs:comment xml:lang="en">JavaLibrary implementing the org.omg.PortableServer package for J2SE 1.4</rdfs:comment>
		<rdfs:comment xml:lang="OWLManchester">platform:implementsInterface some OrgOmgPortableServerAPI</rdfs:comment>
	</owl:Class>
	<owl:Class rdf:about="&j2se-1_4;OrgOmgPortableServerCurrentPackageClassLibrary">
		<rdfs:subClassOf rdf:resource="&java;JavaClassLibrary"/>
		<rdfs:comment xml:lang="en">JavaLibrary implementing the org.omg.PortableServer.CurrentPackage package for J2SE 1.4</rdfs:comment>
		<rdfs:comment xml:lang="OWLManchester">platform:implementsInterface some OrgOmgPortableServerCurrentPackageAPI</rdfs:comment>
	</owl:Class>
	<owl:Class rdf:about="&j2se-1_4;OrgOmgPortableServerPOAManagerPackageClassLibrary">
		<rdfs:subClassOf rdf:resource="&java;JavaClassLibrary"/>
		<rdfs:comment xml:lang="en">JavaLibrary implementing the org.omg.PortableServer.POAManagerPackage package for J2SE 1.4</rdfs:comment>
		<rdfs:comment xml:lang="OWLManchester">platform:implementsInterface some OrgOmgPortableServerPOAManagerPackageAPI</rdfs:comment>
	</owl:Class>
	<owl:Class rdf:about="&j2se-1_4;OrgOmgPortableServerPOAPackageClassLibrary">
		<rdfs:subClassOf rdf:resource="&java;JavaClassLibrary"/>
		<rdfs:comment xml:lang="en">JavaLibrary implementing the org.omg.PortableServer.POAPackage package for J2SE 1.4</rdfs:comment>
		<rdfs:comment xml:lang="OWLManchester">platform:implementsInterface some OrgOmgPortableServerPOAPackageAPI</rdfs:comment>
	</owl:Class>
	<owl:Class rdf:about="&j2se-1_4;OrgOmgPortableServerPortableClassLibrary">
		<rdfs:subClassOf rdf:resource="&java;JavaClassLibrary"/>
		<rdfs:comment xml:lang="en">JavaLibrary implementing the org.omg.PortableServer.portable package for J2SE 1.4</rdfs:comment>
		<rdfs:comment xml:lang="OWLManchester">platform:implementsInterface some OrgOmgPortableServerPortableAPI</rdfs:comment>
	</owl:Class>
	<owl:Class rdf:about="&j2se-1_4;OrgOmgPortableServerServantLocatorPackageClassLibrary">
		<rdfs:subClassOf rdf:resource="&java;JavaClassLibrary"/>
		<rdfs:comment xml:lang="en">JavaLibrary implementing the org.omg.PortableServer.ServantLocatorPackage package for J2SE 1.4</rdfs:comment>
		<rdfs:comment xml:lang="OWLManchester">platform:implementsInterface some OrgOmgPortableServerServantLocatorPackageAPI</rdfs:comment>
	</owl:Class>
	<owl:Class rdf:about="&j2se-1_4;OrgOmgDynamicClassLibrary">
		<rdfs:subClassOf rdf:resource="&java;JavaClassLibrary"/>
		<rdfs:comment xml:lang="en">JavaLibrary implementing the org.omg.Dynamic package for J2SE 1.4</rdfs:comment>
		<rdfs:comment xml:lang="OWLManchester">platform:implementsInterface some OrgOmgDynamicAPI</rdfs:comment>
	</owl:Class>
	<owl:Class rdf:about="&j2se-1_4;OrgOmgDynamicAnyClassLibrary">
		<rdfs:subClassOf rdf:resource="&java;JavaClassLibrary"/>
		<rdfs:comment xml:lang="en">JavaLibrary implementing the org.omg.DynamicAny package for J2SE 1.4</rdfs:comment>
		<rdfs:comment xml:lang="OWLManchester">platform:implementsInterface some OrgOmgDynamicAnyAPI</rdfs:comment>
	</owl:Class>
	<owl:Class rdf:about="&j2se-1_4;OrgOmgDynamicAnyDynAnyFactoryPackageClassLibrary">
		<rdfs:subClassOf rdf:resource="&java;JavaClassLibrary"/>
		<rdfs:comment xml:lang="en">JavaLibrary implementing the org.omg.DynamicAny.DynAnyFactoryPackage package for J2SE 1.4</rdfs:comment>
		<rdfs:comment xml:lang="OWLManchester">platform:implementsInterface some OrgOmgDynamicAnyDynAnyFactoryPackageAPI</rdfs:comment>
	</owl:Class>
	<owl:Class rdf:about="&j2se-1_4;OrgOmgDynamicAnyDynAnyPackageClassLibrary">
		<rdfs:subClassOf rdf:resource="&java;JavaClassLibrary"/>
		<rdfs:comment xml:lang="en">JavaLibrary implementing the org.omg.DynamicAny.DynAnyPackage package for J2SE 1.4</rdfs:comment>
		<rdfs:comment xml:lang="OWLManchester">platform:implementsInterface some OrgOmgDynamicAnyDynAnyPackageAPI</rdfs:comment>
	</owl:Class>
	<owl:Class rdf:about="&j2se-1_4;OrgOmgIOPClassLibrary">
		<rdfs:subClassOf rdf:resource="&java;JavaClassLibrary"/>
		<rdfs:comment xml:lang="en">JavaLibrary implementing the org.omg.IOP package for J2SE 1.4</rdfs:comment>
		<rdfs:comment xml:lang="OWLManchester">platform:implementsInterface some OrgOmgIOPAPI</rdfs:comment>
	</owl:Class>
	<owl:Class rdf:about="&j2se-1_4;OrgOmgIOPCodecFactoryPackageClassLibrary">
		<rdfs:subClassOf rdf:resource="&java;JavaClassLibrary"/>
		<rdfs:comment xml:lang="en">JavaLibrary implementing the org.omg.IOP.CodecFactoryPackage package for J2SE 1.4</rdfs:comment>
		<rdfs:comment xml:lang="OWLManchester">platform:implementsInterface some OrgOmgIOPCodecFactoryPackageAPI</rdfs:comment>
	</owl:Class>
	<owl:Class rdf:about="&j2se-1_4;OrgOmgIOPCodecPackageClassLibrary">
		<rdfs:subClassOf rdf:resource="&java;JavaClassLibrary"/>
		<rdfs:comment xml:lang="en">JavaLibrary implementing the org.omg.IOP.CodecPackage package for J2SE 1.4</rdfs:comment>
		<rdfs:comment xml:lang="OWLManchester">platform:implementsInterface some OrgOmgIOPCodecPackageAPI</rdfs:comment>
	</owl:Class>
	<owl:Class rdf:about="&j2se-1_4;OrgOmgMessagingClassLibrary">
		<rdfs:subClassOf rdf:resource="&java;JavaClassLibrary"/>
		<rdfs:comment xml:lang="en">JavaLibrary implementing the org.omg.Messaging package for J2SE 1.4</rdfs:comment>
		<rdfs:comment xml:lang="OWLManchester">platform:implementsInterface some OrgOmgMessagingAPI</rdfs:comment>
	</owl:Class>
	<owl:Class rdf:about="&j2se-1_4;OrgOmgPortableInterceptorClassLibrary">
		<rdfs:subClassOf rdf:resource="&java;JavaClassLibrary"/>
		<rdfs:comment xml:lang="en">JavaLibrary implementing the org.omg.PortableInterceptor package for J2SE 1.4</rdfs:comment>
		<rdfs:comment xml:lang="OWLManchester">platform:implementsInterface some OrgOmgPortableInterceptorAPI</rdfs:comment>
	</owl:Class>
	<owl:Class rdf:about="&j2se-1_4;OrgOmgPortableInterceptorORBInitInfoPackageClassLibrary">
		<rdfs:subClassOf rdf:resource="&java;JavaClassLibrary"/>
		<rdfs:comment xml:lang="en">JavaLibrary implementing the org.omg.PortableInterceptor.ORBInitInfoPackage package for J2SE 1.4</rdfs:comment>
		<rdfs:comment xml:lang="OWLManchester">platform:implementsInterface some OrgOmgPortableInterceptorORBInitInfoPackageAPI</rdfs:comment>
	</owl:Class>
	<owl:Class rdf:about="&j2se-1_4;OrgOmgStubJavaRmiClassLibrary">
		<owl:equivalentClass rdf:resource="&j2se-1_3;OrgOmgStubJavaRmiClassLibrary"/>
		<rdfs:subClassOf rdf:resource="&java;JavaClassLibrary"/>
		<rdfs:comment xml:lang="en">JavaLibrary implementing the org.omg.stub.java.rmi package for J2SE 1.4</rdfs:comment>
		<rdfs:comment xml:lang="OWLManchester">platform:implementsInterface some OrgOmgStubJavaRmiAPI</rdfs:comment>
	</owl:Class>
	<owl:Class rdf:about="&j2se-1_4;OrgXmlSaxClassLibrary">
		<rdfs:subClassOf rdf:resource="&java;JavaClassLibrary"/>
		<rdfs:comment xml:lang="en">JavaLibrary implementing the org.xml.sax package for J2SE 1.4</rdfs:comment>
		<rdfs:comment xml:lang="OWLManchester">platform:implementsInterface some OrgXmlSaxAPI</rdfs:comment>
	</owl:Class>
	<owl:Class rdf:about="&j2se-1_4;OrgXmlSaxHelpersClassLibrary">
		<rdfs:subClassOf rdf:resource="&java;JavaClassLibrary"/>
		<rdfs:comment xml:lang="en">JavaLibrary implementing the org.xml.sax.helpers package for J2SE 1.4</rdfs:comment>
		<rdfs:comment xml:lang="OWLManchester">platform:implementsInterface some OrgXmlSaxHelpersAPI</rdfs:comment>
	</owl:Class>
	<owl:Class rdf:about="&j2se-1_4;OrgXmlSaxExtClassLibrary">
		<rdfs:subClassOf rdf:resource="&java;JavaClassLibrary"/>
		<rdfs:comment xml:lang="en">JavaLibrary implementing the org.xml.sax.ext package for J2SE 1.4</rdfs:comment>
		<rdfs:comment xml:lang="OWLManchester">platform:implementsInterface some OrgXmlSaxExtAPI</rdfs:comment>
	</owl:Class>
	<owl:Class rdf:about="&j2se-1_4;OrgIetfJgssClassLibrary">
		<rdfs:subClassOf rdf:resource="&java;JavaClassLibrary"/>
		<rdfs:comment xml:lang="en">JavaLibrary implementing the org.ietf.jgss package for J2SE 1.4</rdfs:comment>
		<rdfs:comment xml:lang="OWLManchester">platform:implementsInterface some OrgIetfJgssAPI</rdfs:comment>
	</owl:Class>
</rdf:RDF>
