<?xml version="1.0" encoding="ISO-8859-1"?>
<!DOCTYPE rdf:RDF [
	<!ENTITY isa "http://localhost/~dennis/platformkit/2010_1/isa.owl#">
	<!ENTITY j2me-pp-1_0 "http://soft.vub.ac.be/platformkit/2010/1/j2me-pp-1_0.owl#">
	<!ENTITY j2se-1_3 "http://soft.vub.ac.be/platformkit/2010/1/j2se-1_3.owl#">
	<!ENTITY xsd "http://www.w3.org/2001/XMLSchema#">
	<!ENTITY j2se-1_2 "http://soft.vub.ac.be/platformkit/2010/1/j2se-1_2.owl#">
	<!ENTITY java "http://localhost/~dennis/platformkit/2010_1/java.owl#">
	<!ENTITY ns_19 "http://localhost/~dennis/platformkit/2010_1/">
	<!ENTITY platform "http://localhost/~dennis/platformkit/2010_1/platform.owl#">
	<!ENTITY rdf "http://www.w3.org/1999/02/22-rdf-syntax-ns#">
	<!ENTITY rdfs "http://www.w3.org/2000/01/rdf-schema#">
	<!ENTITY owl "http://www.w3.org/2002/07/owl#">
]>
<rdf:RDF
	 xmlns:isa="&isa;"
	 xmlns:j2me-pp-1_0="&j2me-pp-1_0;"
	 xmlns:j2se-1_3="&j2se-1_3;"
	 xmlns:xsd="&xsd;"
	 xmlns:j2se-1_2="&j2se-1_2;"
	 xmlns:java="&java;"
	 xmlns:ns_19="&ns_19;"
	 xmlns:platform="&platform;"
	 xmlns:rdf="&rdf;"
	 xmlns:rdfs="&rdfs;"
	 xmlns:owl="&owl;"
>

	<owl:Ontology rdf:about="http://soft.vub.ac.be/platformkit/2010/1/j2se-1_3.owl#">
		<owl:versionInfo>$Id: UML2ToPackageAPIOntology.atl 8082 2010-03-18 21:11:00Z dwagelaa $</owl:versionInfo>
		<owl:imports rdf:resource="http://localhost/~dennis/platformkit/2010_1/platform.owl"/>
		<owl:imports rdf:resource="http://localhost/~dennis/platformkit/2010_1/java.owl"/>
		<owl:imports rdf:resource="http://soft.vub.ac.be/platformkit/2010/1/j2se-1_2.owl#"/>
		<owl:imports rdf:resource="http://localhost/~dennis/platformkit/2010_1/isa.owl"/>
		<owl:imports rdf:resource="http://soft.vub.ac.be/platformkit/2010/1/j2me-pp-1_0.owl#"/>
		<rdfs:comment xml:lang="en">Generated by [UML2ToSimplifiedPackageAPIOntology.atl 8080 2010-03-18 10:46:40Z dwagelaa], [UML2ToPackageAPIOntology.atl 8082 2010-03-18 21:11:00Z dwagelaa], [UML2ToAPIOntology.atl 8082 2010-03-18 21:11:00Z dwagelaa], and [UML2Comparison.atl 8082 2010-03-18 21:11:00Z dwagelaa]</rdfs:comment>
		<rdfs:comment>Dennis Wagelaar &lt;dennis.wagelaar@vub.ac.be&gt;</rdfs:comment>
		<rdfs:comment xml:lang="en">&#169; 2010, Vrije Universiteit Brussel. All rights reserved.</rdfs:comment>
		<rdfs:label xml:lang="en">J2SE 1.3</rdfs:label>
	</owl:Ontology>
	<owl:Class rdf:about="&j2se-1_3;J2SE1_3API">
		<rdfs:subClassOf rdf:resource="&j2se-1_3;JavaIoAPI"/>
		<rdfs:subClassOf rdf:resource="&j2se-1_3;JavaLangAPI"/>
		<rdfs:subClassOf rdf:resource="&j2se-1_3;JavaLangReflectAPI"/>
		<rdfs:subClassOf rdf:resource="&j2se-1_3;JavaLangRefAPI"/>
		<rdfs:subClassOf rdf:resource="&j2se-1_3;JavaNetAPI"/>
		<rdfs:subClassOf rdf:resource="&j2se-1_3;JavaSecurityAPI"/>
		<rdfs:subClassOf rdf:resource="&j2se-1_3;JavaSecurityCertAPI"/>
		<rdfs:subClassOf rdf:resource="&j2se-1_3;JavaSecuritySpecAPI"/>
		<rdfs:subClassOf rdf:resource="&j2se-1_3;JavaSecurityInterfacesAPI"/>
		<rdfs:subClassOf rdf:resource="&j2se-1_3;JavaSecurityAclAPI"/>
		<rdfs:subClassOf rdf:resource="&j2se-1_3;JavaUtilAPI"/>
		<rdfs:subClassOf rdf:resource="&j2se-1_3;JavaUtilJarAPI"/>
		<rdfs:subClassOf rdf:resource="&j2se-1_3;JavaUtilZipAPI"/>
		<rdfs:subClassOf rdf:resource="&j2se-1_3;JavaMathAPI"/>
		<rdfs:subClassOf rdf:resource="&j2se-1_3;JavaTextAPI"/>
		<rdfs:subClassOf rdf:resource="&j2se-1_3;JavaTextResourcesAPI"/>
		<rdfs:subClassOf rdf:resource="&j2se-1_3;JavaAwtAPI"/>
		<rdfs:subClassOf rdf:resource="&j2se-1_3;JavaAwtGeomAPI"/>
		<rdfs:subClassOf rdf:resource="&j2se-1_3;JavaAwtEventAPI"/>
		<rdfs:subClassOf rdf:resource="&j2se-1_3;JavaAwtFontAPI"/>
		<rdfs:subClassOf rdf:resource="&j2se-1_3;JavaAwtImageAPI"/>
		<rdfs:subClassOf rdf:resource="&j2se-1_3;JavaAwtImageRenderableAPI"/>
		<rdfs:subClassOf rdf:resource="&j2se-1_3;JavaAwtDndAPI"/>
		<rdfs:subClassOf rdf:resource="&j2se-1_3;JavaAwtImAPI"/>
		<rdfs:subClassOf rdf:resource="&j2se-1_3;JavaAwtImSpiAPI"/>
		<rdfs:subClassOf rdf:resource="&j2se-1_3;JavaAwtColorAPI"/>
		<rdfs:subClassOf rdf:resource="&j2se-1_3;JavaAwtDatatransferAPI"/>
		<rdfs:subClassOf rdf:resource="&j2se-1_3;JavaAwtPrintAPI"/>
		<rdfs:subClassOf rdf:resource="&j2se-1_3;JavaBeansAPI"/>
		<rdfs:subClassOf rdf:resource="&j2se-1_3;JavaBeansBeancontextAPI"/>
		<rdfs:subClassOf rdf:resource="&j2se-1_3;JavaAppletAPI"/>
		<rdfs:subClassOf rdf:resource="&j2se-1_3;JavaRmiAPI"/>
		<rdfs:subClassOf rdf:resource="&j2se-1_3;JavaRmiServerAPI"/>
		<rdfs:subClassOf rdf:resource="&j2se-1_3;JavaRmiDgcAPI"/>
		<rdfs:subClassOf rdf:resource="&j2se-1_3;JavaRmiRegistryAPI"/>
		<rdfs:subClassOf rdf:resource="&j2se-1_3;JavaRmiActivationAPI"/>
		<rdfs:subClassOf rdf:resource="&j2se-1_3;JavaSqlAPI"/>
		<rdfs:subClassOf rdf:resource="&j2se-1_3;JavaxAccessibilityAPI"/>
		<rdfs:subClassOf rdf:resource="&j2se-1_3;JavaxSwingAPI"/>
		<rdfs:subClassOf rdf:resource="&j2se-1_3;JavaxSwingTextAPI"/>
		<rdfs:subClassOf rdf:resource="&j2se-1_3;JavaxSwingTextHtmlAPI"/>
		<rdfs:subClassOf rdf:resource="&j2se-1_3;JavaxSwingTextHtmlParserAPI"/>
		<rdfs:subClassOf rdf:resource="&j2se-1_3;JavaxSwingTextRtfAPI"/>
		<rdfs:subClassOf rdf:resource="&j2se-1_3;JavaxSwingEventAPI"/>
		<rdfs:subClassOf rdf:resource="&j2se-1_3;JavaxSwingPlafAPI"/>
		<rdfs:subClassOf rdf:resource="&j2se-1_3;JavaxSwingPlafBasicAPI"/>
		<rdfs:subClassOf rdf:resource="&j2se-1_3;JavaxSwingPlafMetalAPI"/>
		<rdfs:subClassOf rdf:resource="&j2se-1_3;JavaxSwingPlafMultiAPI"/>
		<rdfs:subClassOf rdf:resource="&j2se-1_3;JavaxSwingUndoAPI"/>
		<rdfs:subClassOf rdf:resource="&j2se-1_3;JavaxSwingTreeAPI"/>
		<rdfs:subClassOf rdf:resource="&j2se-1_3;JavaxSwingTableAPI"/>
		<rdfs:subClassOf rdf:resource="&j2se-1_3;JavaxSwingBorderAPI"/>
		<rdfs:subClassOf rdf:resource="&j2se-1_3;JavaxSwingColorchooserAPI"/>
		<rdfs:subClassOf rdf:resource="&j2se-1_3;JavaxSwingFilechooserAPI"/>
		<rdfs:subClassOf rdf:resource="&j2se-1_3;JavaxNamingAPI"/>
		<rdfs:subClassOf rdf:resource="&j2se-1_3;JavaxNamingDirectoryAPI"/>
		<rdfs:subClassOf rdf:resource="&j2se-1_3;JavaxNamingEventAPI"/>
		<rdfs:subClassOf rdf:resource="&j2se-1_3;JavaxNamingLdapAPI"/>
		<rdfs:subClassOf rdf:resource="&j2se-1_3;JavaxNamingSpiAPI"/>
		<rdfs:subClassOf rdf:resource="&j2se-1_3;JavaxSoundMidiAPI"/>
		<rdfs:subClassOf rdf:resource="&j2se-1_3;JavaxSoundMidiSpiAPI"/>
		<rdfs:subClassOf rdf:resource="&j2se-1_3;JavaxSoundSampledAPI"/>
		<rdfs:subClassOf rdf:resource="&j2se-1_3;JavaxSoundSampledSpiAPI"/>
		<rdfs:subClassOf rdf:resource="&j2se-1_3;JavaxRmiAPI"/>
		<rdfs:subClassOf rdf:resource="&j2se-1_3;JavaxRmiCORBAAPI"/>
		<rdfs:subClassOf rdf:resource="&j2se-1_3;JavaxTransactionAPI"/>
		<rdfs:subClassOf rdf:resource="&j2se-1_3;OrgOmgCORBA_2_3API"/>
		<rdfs:subClassOf rdf:resource="&j2se-1_3;OrgOmgCORBA_2_3PortableAPI"/>
		<rdfs:subClassOf rdf:resource="&j2se-1_3;OrgOmgCORBAAPI"/>
		<rdfs:subClassOf rdf:resource="&j2se-1_3;OrgOmgCORBAPortableAPI"/>
		<rdfs:subClassOf rdf:resource="&j2se-1_3;OrgOmgCORBATypeCodePackageAPI"/>
		<rdfs:subClassOf rdf:resource="&j2se-1_3;OrgOmgCORBAORBPackageAPI"/>
		<rdfs:subClassOf rdf:resource="&j2se-1_3;OrgOmgCORBADynAnyPackageAPI"/>
		<rdfs:subClassOf rdf:resource="&j2se-1_3;OrgOmgSendingContextAPI"/>
		<rdfs:subClassOf rdf:resource="&j2se-1_3;OrgOmgCosNamingAPI"/>
		<rdfs:subClassOf rdf:resource="&j2se-1_3;OrgOmgCosNamingNamingContextPackageAPI"/>
		<rdfs:subClassOf rdf:resource="&j2se-1_3;OrgOmgStubJavaRmiAPI"/>
		<rdfs:comment xml:lang="en">J2SE 1.3 API</rdfs:comment>
		<rdfs:comment xml:lang="OWLManchester">platform:comprisesInterfacePart some JavaIo and platform:comprisesInterfacePart some JavaLang and platform:comprisesInterfacePart some JavaLangReflect and platform:comprisesInterfacePart some JavaLangRef and platform:comprisesInterfacePart some JavaNet and platform:comprisesInterfacePart some JavaSecurity and platform:comprisesInterfacePart some JavaSecurityCert and platform:comprisesInterfacePart some JavaSecuritySpec and platform:comprisesInterfacePart some JavaSecurityInterfaces and platform:comprisesInterfacePart some JavaSecurityAcl and platform:comprisesInterfacePart some JavaUtil and platform:comprisesInterfacePart some JavaUtilJar and platform:comprisesInterfacePart some JavaUtilZip and platform:comprisesInterfacePart some JavaMath and platform:comprisesInterfacePart some JavaText and platform:comprisesInterfacePart some JavaTextResources and platform:comprisesInterfacePart some JavaAwt and platform:comprisesInterfacePart some JavaAwtGeom and platform:comprisesInterfacePart some JavaAwtEvent and platform:comprisesInterfacePart some JavaAwtFont and platform:comprisesInterfacePart some JavaAwtImage and platform:comprisesInterfacePart some JavaAwtImageRenderable and platform:comprisesInterfacePart some JavaAwtDnd and platform:comprisesInterfacePart some JavaAwtIm and platform:comprisesInterfacePart some JavaAwtImSpi and platform:comprisesInterfacePart some JavaAwtColor and platform:comprisesInterfacePart some JavaAwtDatatransfer and platform:comprisesInterfacePart some JavaAwtPrint and platform:comprisesInterfacePart some JavaBeans and platform:comprisesInterfacePart some JavaBeansBeancontext and platform:comprisesInterfacePart some JavaApplet and platform:comprisesInterfacePart some JavaRmi and platform:comprisesInterfacePart some JavaRmiServer and platform:comprisesInterfacePart some JavaRmiDgc and platform:comprisesInterfacePart some JavaRmiRegistry and platform:comprisesInterfacePart some JavaRmiActivation and platform:comprisesInterfacePart some JavaSql and platform:comprisesInterfacePart some JavaxAccessibility and platform:comprisesInterfacePart some JavaxSwing and platform:comprisesInterfacePart some JavaxSwingText and platform:comprisesInterfacePart some JavaxSwingTextHtml and platform:comprisesInterfacePart some JavaxSwingTextHtmlParser and platform:comprisesInterfacePart some JavaxSwingTextRtf and platform:comprisesInterfacePart some JavaxSwingEvent and platform:comprisesInterfacePart some JavaxSwingPlaf and platform:comprisesInterfacePart some JavaxSwingPlafBasic and platform:comprisesInterfacePart some JavaxSwingPlafMetal and platform:comprisesInterfacePart some JavaxSwingPlafMulti and platform:comprisesInterfacePart some JavaxSwingUndo and platform:comprisesInterfacePart some JavaxSwingTree and platform:comprisesInterfacePart some JavaxSwingTable and platform:comprisesInterfacePart some JavaxSwingBorder and platform:comprisesInterfacePart some JavaxSwingColorchooser and platform:comprisesInterfacePart some JavaxSwingFilechooser and platform:comprisesInterfacePart some JavaxNaming and platform:comprisesInterfacePart some JavaxNamingDirectory and platform:comprisesInterfacePart some JavaxNamingEvent and platform:comprisesInterfacePart some JavaxNamingLdap and platform:comprisesInterfacePart some JavaxNamingSpi and platform:comprisesInterfacePart some JavaxSoundMidi and platform:comprisesInterfacePart some JavaxSoundMidiSpi and platform:comprisesInterfacePart some JavaxSoundSampled and platform:comprisesInterfacePart some JavaxSoundSampledSpi and platform:comprisesInterfacePart some JavaxRmi and platform:comprisesInterfacePart some JavaxRmiCORBA and platform:comprisesInterfacePart some JavaxTransaction and platform:comprisesInterfacePart some OrgOmgCORBA_2_3 and platform:comprisesInterfacePart some OrgOmgCORBA_2_3Portable and platform:comprisesInterfacePart some OrgOmgCORBA and platform:comprisesInterfacePart some OrgOmgCORBAPortable and platform:comprisesInterfacePart some OrgOmgCORBATypeCodePackage and platform:comprisesInterfacePart some OrgOmgCORBAORBPackage and platform:comprisesInterfacePart some OrgOmgCORBADynAnyPackage and platform:comprisesInterfacePart some OrgOmgSendingContext and platform:comprisesInterfacePart some OrgOmgCosNaming and platform:comprisesInterfacePart some OrgOmgCosNamingNamingContextPackage and platform:comprisesInterfacePart some OrgOmgStubJavaRmi</rdfs:comment>
	</owl:Class>
	<owl:Class rdf:about="&j2se-1_3;J2SE1_3ClassLibrary">
		<rdfs:subClassOf rdf:resource="&j2se-1_3;JavaIoClassLibrary"/>
		<rdfs:subClassOf rdf:resource="&j2se-1_3;JavaLangClassLibrary"/>
		<rdfs:subClassOf rdf:resource="&j2se-1_3;JavaLangReflectClassLibrary"/>
		<rdfs:subClassOf rdf:resource="&j2se-1_3;JavaLangRefClassLibrary"/>
		<rdfs:subClassOf rdf:resource="&j2se-1_3;JavaNetClassLibrary"/>
		<rdfs:subClassOf rdf:resource="&j2se-1_3;JavaSecurityClassLibrary"/>
		<rdfs:subClassOf rdf:resource="&j2se-1_3;JavaSecurityCertClassLibrary"/>
		<rdfs:subClassOf rdf:resource="&j2se-1_3;JavaSecuritySpecClassLibrary"/>
		<rdfs:subClassOf rdf:resource="&j2se-1_3;JavaSecurityInterfacesClassLibrary"/>
		<rdfs:subClassOf rdf:resource="&j2se-1_3;JavaSecurityAclClassLibrary"/>
		<rdfs:subClassOf rdf:resource="&j2se-1_3;JavaUtilClassLibrary"/>
		<rdfs:subClassOf rdf:resource="&j2se-1_3;JavaUtilJarClassLibrary"/>
		<rdfs:subClassOf rdf:resource="&j2se-1_3;JavaUtilZipClassLibrary"/>
		<rdfs:subClassOf rdf:resource="&j2se-1_3;JavaMathClassLibrary"/>
		<rdfs:subClassOf rdf:resource="&j2se-1_3;JavaTextClassLibrary"/>
		<rdfs:subClassOf rdf:resource="&j2se-1_3;JavaTextResourcesClassLibrary"/>
		<rdfs:subClassOf rdf:resource="&j2se-1_3;JavaAwtClassLibrary"/>
		<rdfs:subClassOf rdf:resource="&j2se-1_3;JavaAwtGeomClassLibrary"/>
		<rdfs:subClassOf rdf:resource="&j2se-1_3;JavaAwtEventClassLibrary"/>
		<rdfs:subClassOf rdf:resource="&j2se-1_3;JavaAwtFontClassLibrary"/>
		<rdfs:subClassOf rdf:resource="&j2se-1_3;JavaAwtImageClassLibrary"/>
		<rdfs:subClassOf rdf:resource="&j2se-1_3;JavaAwtImageRenderableClassLibrary"/>
		<rdfs:subClassOf rdf:resource="&j2se-1_3;JavaAwtDndClassLibrary"/>
		<rdfs:subClassOf rdf:resource="&j2se-1_3;JavaAwtImClassLibrary"/>
		<rdfs:subClassOf rdf:resource="&j2se-1_3;JavaAwtImSpiClassLibrary"/>
		<rdfs:subClassOf rdf:resource="&j2se-1_3;JavaAwtColorClassLibrary"/>
		<rdfs:subClassOf rdf:resource="&j2se-1_3;JavaAwtDatatransferClassLibrary"/>
		<rdfs:subClassOf rdf:resource="&j2se-1_3;JavaAwtPrintClassLibrary"/>
		<rdfs:subClassOf rdf:resource="&j2se-1_3;JavaBeansClassLibrary"/>
		<rdfs:subClassOf rdf:resource="&j2se-1_3;JavaBeansBeancontextClassLibrary"/>
		<rdfs:subClassOf rdf:resource="&j2se-1_3;JavaAppletClassLibrary"/>
		<rdfs:subClassOf rdf:resource="&j2se-1_3;JavaRmiClassLibrary"/>
		<rdfs:subClassOf rdf:resource="&j2se-1_3;JavaRmiServerClassLibrary"/>
		<rdfs:subClassOf rdf:resource="&j2se-1_3;JavaRmiDgcClassLibrary"/>
		<rdfs:subClassOf rdf:resource="&j2se-1_3;JavaRmiRegistryClassLibrary"/>
		<rdfs:subClassOf rdf:resource="&j2se-1_3;JavaRmiActivationClassLibrary"/>
		<rdfs:subClassOf rdf:resource="&j2se-1_3;JavaSqlClassLibrary"/>
		<rdfs:subClassOf rdf:resource="&j2se-1_3;JavaxAccessibilityClassLibrary"/>
		<rdfs:subClassOf rdf:resource="&j2se-1_3;JavaxSwingClassLibrary"/>
		<rdfs:subClassOf rdf:resource="&j2se-1_3;JavaxSwingTextClassLibrary"/>
		<rdfs:subClassOf rdf:resource="&j2se-1_3;JavaxSwingTextHtmlClassLibrary"/>
		<rdfs:subClassOf rdf:resource="&j2se-1_3;JavaxSwingTextHtmlParserClassLibrary"/>
		<rdfs:subClassOf rdf:resource="&j2se-1_3;JavaxSwingTextRtfClassLibrary"/>
		<rdfs:subClassOf rdf:resource="&j2se-1_3;JavaxSwingEventClassLibrary"/>
		<rdfs:subClassOf rdf:resource="&j2se-1_3;JavaxSwingPlafClassLibrary"/>
		<rdfs:subClassOf rdf:resource="&j2se-1_3;JavaxSwingPlafBasicClassLibrary"/>
		<rdfs:subClassOf rdf:resource="&j2se-1_3;JavaxSwingPlafMetalClassLibrary"/>
		<rdfs:subClassOf rdf:resource="&j2se-1_3;JavaxSwingPlafMultiClassLibrary"/>
		<rdfs:subClassOf rdf:resource="&j2se-1_3;JavaxSwingUndoClassLibrary"/>
		<rdfs:subClassOf rdf:resource="&j2se-1_3;JavaxSwingTreeClassLibrary"/>
		<rdfs:subClassOf rdf:resource="&j2se-1_3;JavaxSwingTableClassLibrary"/>
		<rdfs:subClassOf rdf:resource="&j2se-1_3;JavaxSwingBorderClassLibrary"/>
		<rdfs:subClassOf rdf:resource="&j2se-1_3;JavaxSwingColorchooserClassLibrary"/>
		<rdfs:subClassOf rdf:resource="&j2se-1_3;JavaxSwingFilechooserClassLibrary"/>
		<rdfs:subClassOf rdf:resource="&j2se-1_3;JavaxNamingClassLibrary"/>
		<rdfs:subClassOf rdf:resource="&j2se-1_3;JavaxNamingDirectoryClassLibrary"/>
		<rdfs:subClassOf rdf:resource="&j2se-1_3;JavaxNamingEventClassLibrary"/>
		<rdfs:subClassOf rdf:resource="&j2se-1_3;JavaxNamingLdapClassLibrary"/>
		<rdfs:subClassOf rdf:resource="&j2se-1_3;JavaxNamingSpiClassLibrary"/>
		<rdfs:subClassOf rdf:resource="&j2se-1_3;JavaxSoundMidiClassLibrary"/>
		<rdfs:subClassOf rdf:resource="&j2se-1_3;JavaxSoundMidiSpiClassLibrary"/>
		<rdfs:subClassOf rdf:resource="&j2se-1_3;JavaxSoundSampledClassLibrary"/>
		<rdfs:subClassOf rdf:resource="&j2se-1_3;JavaxSoundSampledSpiClassLibrary"/>
		<rdfs:subClassOf rdf:resource="&j2se-1_3;JavaxRmiClassLibrary"/>
		<rdfs:subClassOf rdf:resource="&j2se-1_3;JavaxRmiCORBAClassLibrary"/>
		<rdfs:subClassOf rdf:resource="&j2se-1_3;JavaxTransactionClassLibrary"/>
		<rdfs:subClassOf rdf:resource="&j2se-1_3;OrgOmgCORBA_2_3ClassLibrary"/>
		<rdfs:subClassOf rdf:resource="&j2se-1_3;OrgOmgCORBA_2_3PortableClassLibrary"/>
		<rdfs:subClassOf rdf:resource="&j2se-1_3;OrgOmgCORBAClassLibrary"/>
		<rdfs:subClassOf rdf:resource="&j2se-1_3;OrgOmgCORBAPortableClassLibrary"/>
		<rdfs:subClassOf rdf:resource="&j2se-1_3;OrgOmgCORBATypeCodePackageClassLibrary"/>
		<rdfs:subClassOf rdf:resource="&j2se-1_3;OrgOmgCORBAORBPackageClassLibrary"/>
		<rdfs:subClassOf rdf:resource="&j2se-1_3;OrgOmgCORBADynAnyPackageClassLibrary"/>
		<rdfs:subClassOf rdf:resource="&j2se-1_3;OrgOmgSendingContextClassLibrary"/>
		<rdfs:subClassOf rdf:resource="&j2se-1_3;OrgOmgCosNamingClassLibrary"/>
		<rdfs:subClassOf rdf:resource="&j2se-1_3;OrgOmgCosNamingNamingContextPackageClassLibrary"/>
		<rdfs:subClassOf rdf:resource="&j2se-1_3;OrgOmgStubJavaRmiClassLibrary"/>
		<rdfs:comment xml:lang="en">Java class library implementing the J2SE 1.3 API</rdfs:comment>
		<rdfs:comment xml:lang="OWLManchester">platform:implementsInterface some J2SE1_3API</rdfs:comment>
	</owl:Class>
	<owl:Class rdf:about="&j2se-1_3;J2SE1_3BytecodeFormat">
		<owl:equivalentClass rdf:resource="&j2me-pp-1_0;J2MEPP1_0BytecodeFormat"/>
		<rdfs:subClassOf rdf:resource="&j2se-1_2;J2SE1_2BytecodeFormat"/>
		<rdfs:comment xml:lang="en">J2SE 1.3 bytecode format</rdfs:comment>
		<rdfs:comment xml:lang="OWLManchester">java:majorVersionNumber some xsd:integer[>="47"^^xsd:integer] and java:preverified value false</rdfs:comment>
	</owl:Class>
	<j2se-1_3:J2SE1_3BytecodeFormat rdf:about="&j2se-1_3;theJ2SE1_3BytecodeFormat">
		<java:preverified rdf:datatype="http://www.w3.org/2001/XMLSchema#boolean">false</java:preverified>
		<java:minorVersionNumber rdf:datatype="http://www.w3.org/2001/XMLSchema#integer">0</java:minorVersionNumber>
		<java:majorVersionNumber rdf:datatype="http://www.w3.org/2001/XMLSchema#integer">47</java:majorVersionNumber>
	</j2se-1_3:J2SE1_3BytecodeFormat>
	<j2se-1_3:J2SE1_3API rdf:about="&j2se-1_3;theJ2SE1_3API">
		<platform:comprisesInterfacePart rdf:resource="&j2se-1_3;theOrgOmgStubJavaRmiPart"/>
		<platform:comprisesInterfacePart rdf:resource="&j2se-1_3;theOrgOmgCosNamingNamingContextPackagePart"/>
		<platform:comprisesInterfacePart rdf:resource="&j2se-1_3;theOrgOmgCosNamingPart"/>
		<platform:comprisesInterfacePart rdf:resource="&j2se-1_3;theOrgOmgSendingContextPart"/>
		<platform:comprisesInterfacePart rdf:resource="&j2se-1_3;theOrgOmgCORBADynAnyPackagePart"/>
		<platform:comprisesInterfacePart rdf:resource="&j2se-1_3;theOrgOmgCORBAORBPackagePart"/>
		<platform:comprisesInterfacePart rdf:resource="&j2se-1_3;theOrgOmgCORBATypeCodePackagePart"/>
		<platform:comprisesInterfacePart rdf:resource="&j2se-1_3;theOrgOmgCORBAPortablePart"/>
		<platform:comprisesInterfacePart rdf:resource="&j2se-1_3;theOrgOmgCORBAPart"/>
		<platform:comprisesInterfacePart rdf:resource="&j2se-1_3;theOrgOmgCORBA_2_3PortablePart"/>
		<platform:comprisesInterfacePart rdf:resource="&j2se-1_3;theOrgOmgCORBA_2_3Part"/>
		<platform:comprisesInterfacePart rdf:resource="&j2se-1_3;theJavaxTransactionPart"/>
		<platform:comprisesInterfacePart rdf:resource="&j2se-1_3;theJavaxRmiCORBAPart"/>
		<platform:comprisesInterfacePart rdf:resource="&j2se-1_3;theJavaxRmiPart"/>
		<platform:comprisesInterfacePart rdf:resource="&j2se-1_3;theJavaxSoundSampledSpiPart"/>
		<platform:comprisesInterfacePart rdf:resource="&j2se-1_3;theJavaxSoundSampledPart"/>
		<platform:comprisesInterfacePart rdf:resource="&j2se-1_3;theJavaxSoundMidiSpiPart"/>
		<platform:comprisesInterfacePart rdf:resource="&j2se-1_3;theJavaxSoundMidiPart"/>
		<platform:comprisesInterfacePart rdf:resource="&j2se-1_3;theJavaxNamingSpiPart"/>
		<platform:comprisesInterfacePart rdf:resource="&j2se-1_3;theJavaxNamingLdapPart"/>
		<platform:comprisesInterfacePart rdf:resource="&j2se-1_3;theJavaxNamingEventPart"/>
		<platform:comprisesInterfacePart rdf:resource="&j2se-1_3;theJavaxNamingDirectoryPart"/>
		<platform:comprisesInterfacePart rdf:resource="&j2se-1_3;theJavaxNamingPart"/>
		<platform:comprisesInterfacePart rdf:resource="&j2se-1_3;theJavaxSwingFilechooserPart"/>
		<platform:comprisesInterfacePart rdf:resource="&j2se-1_3;theJavaxSwingColorchooserPart"/>
		<platform:comprisesInterfacePart rdf:resource="&j2se-1_3;theJavaxSwingBorderPart"/>
		<platform:comprisesInterfacePart rdf:resource="&j2se-1_3;theJavaxSwingTablePart"/>
		<platform:comprisesInterfacePart rdf:resource="&j2se-1_3;theJavaxSwingTreePart"/>
		<platform:comprisesInterfacePart rdf:resource="&j2se-1_3;theJavaxSwingUndoPart"/>
		<platform:comprisesInterfacePart rdf:resource="&j2se-1_3;theJavaxSwingPlafMultiPart"/>
		<platform:comprisesInterfacePart rdf:resource="&j2se-1_3;theJavaxSwingPlafMetalPart"/>
		<platform:comprisesInterfacePart rdf:resource="&j2se-1_3;theJavaxSwingPlafBasicPart"/>
		<platform:comprisesInterfacePart rdf:resource="&j2se-1_3;theJavaxSwingPlafPart"/>
		<platform:comprisesInterfacePart rdf:resource="&j2se-1_3;theJavaxSwingEventPart"/>
		<platform:comprisesInterfacePart rdf:resource="&j2se-1_3;theJavaxSwingTextRtfPart"/>
		<platform:comprisesInterfacePart rdf:resource="&j2se-1_3;theJavaxSwingTextHtmlParserPart"/>
		<platform:comprisesInterfacePart rdf:resource="&j2se-1_3;theJavaxSwingTextHtmlPart"/>
		<platform:comprisesInterfacePart rdf:resource="&j2se-1_3;theJavaxSwingTextPart"/>
		<platform:comprisesInterfacePart rdf:resource="&j2se-1_3;theJavaxSwingPart"/>
		<platform:comprisesInterfacePart rdf:resource="&j2se-1_3;theJavaxAccessibilityPart"/>
		<platform:comprisesInterfacePart rdf:resource="&j2se-1_3;theJavaSqlPart"/>
		<platform:comprisesInterfacePart rdf:resource="&j2se-1_3;theJavaRmiActivationPart"/>
		<platform:comprisesInterfacePart rdf:resource="&j2se-1_3;theJavaRmiRegistryPart"/>
		<platform:comprisesInterfacePart rdf:resource="&j2se-1_3;theJavaRmiDgcPart"/>
		<platform:comprisesInterfacePart rdf:resource="&j2se-1_3;theJavaRmiServerPart"/>
		<platform:comprisesInterfacePart rdf:resource="&j2se-1_3;theJavaRmiPart"/>
		<platform:comprisesInterfacePart rdf:resource="&j2se-1_3;theJavaAppletPart"/>
		<platform:comprisesInterfacePart rdf:resource="&j2se-1_3;theJavaBeansBeancontextPart"/>
		<platform:comprisesInterfacePart rdf:resource="&j2se-1_3;theJavaBeansPart"/>
		<platform:comprisesInterfacePart rdf:resource="&j2se-1_3;theJavaAwtPrintPart"/>
		<platform:comprisesInterfacePart rdf:resource="&j2se-1_3;theJavaAwtDatatransferPart"/>
		<platform:comprisesInterfacePart rdf:resource="&j2se-1_3;theJavaAwtColorPart"/>
		<platform:comprisesInterfacePart rdf:resource="&j2se-1_3;theJavaAwtImSpiPart"/>
		<platform:comprisesInterfacePart rdf:resource="&j2se-1_3;theJavaAwtImPart"/>
		<platform:comprisesInterfacePart rdf:resource="&j2se-1_3;theJavaAwtDndPart"/>
		<platform:comprisesInterfacePart rdf:resource="&j2se-1_3;theJavaAwtImageRenderablePart"/>
		<platform:comprisesInterfacePart rdf:resource="&j2se-1_3;theJavaAwtImagePart"/>
		<platform:comprisesInterfacePart rdf:resource="&j2se-1_3;theJavaAwtFontPart"/>
		<platform:comprisesInterfacePart rdf:resource="&j2se-1_3;theJavaAwtEventPart"/>
		<platform:comprisesInterfacePart rdf:resource="&j2se-1_3;theJavaAwtGeomPart"/>
		<platform:comprisesInterfacePart rdf:resource="&j2se-1_3;theJavaAwtPart"/>
		<platform:comprisesInterfacePart rdf:resource="&j2se-1_3;theJavaTextResourcesPart"/>
		<platform:comprisesInterfacePart rdf:resource="&j2se-1_3;theJavaTextPart"/>
		<platform:comprisesInterfacePart rdf:resource="&j2se-1_3;theJavaMathPart"/>
		<platform:comprisesInterfacePart rdf:resource="&j2se-1_3;theJavaUtilZipPart"/>
		<platform:comprisesInterfacePart rdf:resource="&j2se-1_3;theJavaUtilJarPart"/>
		<platform:comprisesInterfacePart rdf:resource="&j2se-1_3;theJavaUtilPart"/>
		<platform:comprisesInterfacePart rdf:resource="&j2se-1_3;theJavaSecurityAclPart"/>
		<platform:comprisesInterfacePart rdf:resource="&j2se-1_3;theJavaSecurityInterfacesPart"/>
		<platform:comprisesInterfacePart rdf:resource="&j2se-1_3;theJavaSecuritySpecPart"/>
		<platform:comprisesInterfacePart rdf:resource="&j2se-1_3;theJavaSecurityCertPart"/>
		<platform:comprisesInterfacePart rdf:resource="&j2se-1_3;theJavaSecurityPart"/>
		<platform:comprisesInterfacePart rdf:resource="&j2se-1_3;theJavaNetPart"/>
		<platform:comprisesInterfacePart rdf:resource="&j2se-1_3;theJavaLangRefPart"/>
		<platform:comprisesInterfacePart rdf:resource="&j2se-1_3;theJavaLangReflectPart"/>
		<platform:comprisesInterfacePart rdf:resource="&j2se-1_3;theJavaLangPart"/>
		<platform:comprisesInterfacePart rdf:resource="&j2se-1_3;theJavaIoPart"/>
	</j2se-1_3:J2SE1_3API>
	<owl:Class rdf:about="&j2se-1_3;J2SE1_3VM">
		<owl:equivalentClass>
			<owl:Restriction>
				<owl:onProperty rdf:resource="&platform;implementsInterface"/>
				<owl:someValuesFrom rdf:resource="&j2se-1_3;J2SE1_3BytecodeFormat"/>
			</owl:Restriction>
		</owl:equivalentClass>
		<rdfs:subClassOf rdf:resource="&java;JavaVM"/>
		<rdfs:comment xml:lang="en">J2SE 1.3 virtual machine</rdfs:comment>
	</owl:Class>
	<owl:Class rdf:about="&j2se-1_3;J2SE1_3JRE">
		<owl:equivalentClass>
			<owl:Class >
				<owl:intersectionOf rdf:parseType="Collection">
					<owl:Restriction>
						<owl:onProperty rdf:resource="&platform;providesFeature"/>
						<owl:someValuesFrom rdf:resource="&j2se-1_3;J2SE1_3ClassLibrary"/>
					</owl:Restriction>
					<owl:Restriction>
						<owl:onProperty rdf:resource="&platform;providesFeature"/>
						<owl:someValuesFrom rdf:resource="&j2se-1_3;J2SE1_3VM"/>
					</owl:Restriction>
				</owl:intersectionOf>
			</owl:Class>
		</owl:equivalentClass>
		<rdfs:subClassOf rdf:resource="&java;JRE"/>
		<rdfs:comment xml:lang="en">J2SE 1.3 Java Runtime Environment</rdfs:comment>
	</owl:Class>
	<owl:Class rdf:about="&j2se-1_3;JavaIo">
		<rdfs:subClassOf rdf:resource="&j2me-pp-1_0;JavaIo"/>
		<rdfs:subClassOf rdf:resource="&j2se-1_2;JavaIo"/>
		<rdfs:seeAlso rdf:resource="&j2se-1_3;JavaUtil"/>
		<rdfs:seeAlso rdf:resource="&j2se-1_3;JavaNet"/>
		<rdfs:seeAlso rdf:resource="&j2se-1_3;JavaLang"/>
		<rdfs:seeAlso rdf:resource="&j2se-1_3;JavaSecurity"/>
		<rdfs:comment xml:lang="en">Java API part implementing the java.io package for J2SE 1.3</rdfs:comment>
	</owl:Class>
	<owl:Class rdf:about="&j2se-1_3;JavaLang">
		<rdfs:subClassOf rdf:resource="&j2me-pp-1_0;JavaLang"/>
		<rdfs:subClassOf rdf:resource="&j2se-1_2;JavaLang"/>
		<rdfs:seeAlso rdf:resource="&j2se-1_3;JavaLangReflect"/>
		<rdfs:seeAlso rdf:resource="&j2se-1_3;JavaIo"/>
		<rdfs:seeAlso rdf:resource="&j2se-1_3;JavaSecurity"/>
		<rdfs:seeAlso rdf:resource="&j2se-1_3;JavaUtil"/>
		<rdfs:seeAlso rdf:resource="&j2se-1_3;JavaNet"/>
		<rdfs:comment xml:lang="en">Java API part implementing the java.lang package for J2SE 1.3</rdfs:comment>
	</owl:Class>
	<owl:Class rdf:about="&j2se-1_3;JavaLangReflect">
		<owl:equivalentClass rdf:resource="&j2me-pp-1_0;JavaLangReflect"/>
		<rdfs:subClassOf rdf:resource="&j2se-1_2;JavaLangReflect"/>
		<rdfs:seeAlso rdf:resource="&j2se-1_3;JavaLang"/>
		<rdfs:seeAlso rdf:resource="&j2se-1_3;JavaIo"/>
		<rdfs:seeAlso rdf:resource="&j2se-1_3;JavaSecurity"/>
		<rdfs:comment xml:lang="en">Java API part implementing the java.lang.reflect package for J2SE 1.3</rdfs:comment>
	</owl:Class>
	<owl:Class rdf:about="&j2se-1_3;JavaLangRef">
		<owl:equivalentClass rdf:resource="&j2me-pp-1_0;JavaLangRef"/>
		<owl:equivalentClass rdf:resource="&j2se-1_2;JavaLangRef"/>
		<rdfs:subClassOf rdf:resource="&java;JavaAPIPart"/>
		<rdfs:seeAlso rdf:resource="&j2se-1_3;JavaLang"/>
		<rdfs:comment xml:lang="en">Java API part implementing the java.lang.ref package for J2SE 1.3</rdfs:comment>
	</owl:Class>
	<owl:Class rdf:about="&j2se-1_3;JavaNet">
		<rdfs:subClassOf rdf:resource="&j2me-pp-1_0;JavaNet"/>
		<rdfs:subClassOf rdf:resource="&j2se-1_2;JavaNet"/>
		<rdfs:seeAlso rdf:resource="&j2se-1_3;JavaUtilJar"/>
		<rdfs:seeAlso rdf:resource="&j2se-1_3;JavaIo"/>
		<rdfs:seeAlso rdf:resource="&j2se-1_3;JavaSecurity"/>
		<rdfs:seeAlso rdf:resource="&j2se-1_3;JavaUtil"/>
		<rdfs:seeAlso rdf:resource="&j2se-1_3;JavaLang"/>
		<rdfs:comment xml:lang="en">Java API part implementing the java.net package for J2SE 1.3</rdfs:comment>
	</owl:Class>
	<owl:Class rdf:about="&j2se-1_3;JavaSecurity">
		<rdfs:subClassOf rdf:resource="&j2me-pp-1_0;JavaSecurity"/>
		<rdfs:subClassOf rdf:resource="&j2se-1_2;JavaSecurity"/>
		<rdfs:seeAlso rdf:resource="&j2se-1_3;JavaSecuritySpec"/>
		<rdfs:seeAlso rdf:resource="&j2se-1_3;JavaIo"/>
		<rdfs:seeAlso rdf:resource="&j2se-1_3;JavaSecurityCert"/>
		<rdfs:seeAlso rdf:resource="&j2se-1_3;JavaUtil"/>
		<rdfs:seeAlso rdf:resource="&j2se-1_3;JavaNet"/>
		<rdfs:seeAlso rdf:resource="&j2se-1_3;JavaLang"/>
		<rdfs:comment xml:lang="en">Java API part implementing the java.security package for J2SE 1.3</rdfs:comment>
	</owl:Class>
	<owl:Class rdf:about="&j2se-1_3;JavaSecurityCert">
		<owl:equivalentClass rdf:resource="&j2me-pp-1_0;JavaSecurityCert"/>
		<rdfs:subClassOf rdf:resource="&j2se-1_2;JavaSecurityCert"/>
		<rdfs:seeAlso rdf:resource="&j2se-1_3;JavaIo"/>
		<rdfs:seeAlso rdf:resource="&j2se-1_3;JavaSecurity"/>
		<rdfs:seeAlso rdf:resource="&j2se-1_3;JavaMath"/>
		<rdfs:seeAlso rdf:resource="&j2se-1_3;JavaUtil"/>
		<rdfs:seeAlso rdf:resource="&j2se-1_3;JavaLang"/>
		<rdfs:comment xml:lang="en">Java API part implementing the java.security.cert package for J2SE 1.3</rdfs:comment>
	</owl:Class>
	<owl:Class rdf:about="&j2se-1_3;JavaSecuritySpec">
		<owl:equivalentClass rdf:resource="&j2me-pp-1_0;JavaSecuritySpec"/>
		<rdfs:subClassOf rdf:resource="&j2se-1_2;JavaSecuritySpec"/>
		<rdfs:seeAlso rdf:resource="&j2se-1_3;JavaMath"/>
		<rdfs:seeAlso rdf:resource="&j2se-1_3;JavaLang"/>
		<rdfs:seeAlso rdf:resource="&j2se-1_3;JavaSecurity"/>
		<rdfs:seeAlso rdf:resource="&j2se-1_3;JavaSecurityInterfaces"/>
		<rdfs:comment xml:lang="en">Java API part implementing the java.security.spec package for J2SE 1.3</rdfs:comment>
	</owl:Class>
	<owl:Class rdf:about="&j2se-1_3;JavaSecurityInterfaces">
		<owl:equivalentClass rdf:resource="&j2me-pp-1_0;JavaSecurityInterfaces"/>
		<rdfs:subClassOf rdf:resource="&j2se-1_2;JavaSecurityInterfaces"/>
		<rdfs:seeAlso rdf:resource="&j2se-1_3;JavaMath"/>
		<rdfs:seeAlso rdf:resource="&j2se-1_3;JavaSecurity"/>
		<rdfs:comment xml:lang="en">Java API part implementing the java.security.interfaces package for J2SE 1.3</rdfs:comment>
	</owl:Class>
	<owl:Class rdf:about="&j2se-1_3;JavaSecurityAcl">
		<owl:equivalentClass rdf:resource="&j2me-pp-1_0;JavaSecurityAcl"/>
		<owl:equivalentClass rdf:resource="&j2se-1_2;JavaSecurityAcl"/>
		<rdfs:subClassOf rdf:resource="&java;JavaAPIPart"/>
		<rdfs:seeAlso rdf:resource="&j2se-1_3;JavaUtil"/>
		<rdfs:seeAlso rdf:resource="&j2se-1_3;JavaLang"/>
		<rdfs:seeAlso rdf:resource="&j2se-1_3;JavaSecurity"/>
		<rdfs:comment xml:lang="en">Java API part implementing the java.security.acl package for J2SE 1.3</rdfs:comment>
	</owl:Class>
	<owl:Class rdf:about="&j2se-1_3;JavaUtil">
		<rdfs:subClassOf rdf:resource="&j2me-pp-1_0;JavaUtil"/>
		<rdfs:subClassOf rdf:resource="&j2se-1_2;JavaUtil"/>
		<rdfs:seeAlso rdf:resource="&j2se-1_3;JavaIo"/>
		<rdfs:seeAlso rdf:resource="&j2se-1_3;JavaSecurity"/>
		<rdfs:seeAlso rdf:resource="&j2se-1_3;JavaLang"/>
		<rdfs:comment xml:lang="en">Java API part implementing the java.util package for J2SE 1.3</rdfs:comment>
	</owl:Class>
	<owl:Class rdf:about="&j2se-1_3;JavaUtilJar">
		<owl:equivalentClass rdf:resource="&j2me-pp-1_0;JavaUtilJar"/>
		<rdfs:subClassOf rdf:resource="&j2se-1_2;JavaUtilJar"/>
		<rdfs:seeAlso rdf:resource="&j2se-1_3;JavaIo"/>
		<rdfs:seeAlso rdf:resource="&j2se-1_3;JavaUtilZip"/>
		<rdfs:seeAlso rdf:resource="&j2se-1_3;JavaUtil"/>
		<rdfs:seeAlso rdf:resource="&j2se-1_3;JavaLang"/>
		<rdfs:comment xml:lang="en">Java API part implementing the java.util.jar package for J2SE 1.3</rdfs:comment>
	</owl:Class>
	<owl:Class rdf:about="&j2se-1_3;JavaUtilZip">
		<owl:equivalentClass rdf:resource="&j2me-pp-1_0;JavaUtilZip"/>
		<rdfs:subClassOf rdf:resource="&j2se-1_2;JavaUtilZip"/>
		<rdfs:seeAlso rdf:resource="&j2se-1_3;JavaUtil"/>
		<rdfs:seeAlso rdf:resource="&j2se-1_3;JavaLang"/>
		<rdfs:seeAlso rdf:resource="&j2se-1_3;JavaIo"/>
		<rdfs:comment xml:lang="en">Java API part implementing the java.util.zip package for J2SE 1.3</rdfs:comment>
	</owl:Class>
	<owl:Class rdf:about="&j2se-1_3;JavaMath">
		<owl:equivalentClass rdf:resource="&j2me-pp-1_0;JavaMath"/>
		<owl:equivalentClass rdf:resource="&j2se-1_2;JavaMath"/>
		<rdfs:subClassOf rdf:resource="&java;JavaAPIPart"/>
		<rdfs:seeAlso rdf:resource="&j2se-1_3;JavaUtil"/>
		<rdfs:seeAlso rdf:resource="&j2se-1_3;JavaLang"/>
		<rdfs:comment xml:lang="en">Java API part implementing the java.math package for J2SE 1.3</rdfs:comment>
	</owl:Class>
	<owl:Class rdf:about="&j2se-1_3;JavaText">
		<owl:equivalentClass rdf:resource="&j2me-pp-1_0;JavaText"/>
		<rdfs:subClassOf rdf:resource="&java;JavaAPIPart"/>
		<rdfs:seeAlso rdf:resource="&j2se-1_3;JavaIo"/>
		<rdfs:seeAlso rdf:resource="&j2se-1_3;JavaUtil"/>
		<rdfs:seeAlso rdf:resource="&j2se-1_3;JavaLang"/>
		<rdfs:comment xml:lang="en">Java API part implementing the java.text package for J2SE 1.3</rdfs:comment>
	</owl:Class>
	<owl:Class rdf:about="&j2se-1_3;JavaTextResources">
		<owl:equivalentClass rdf:resource="&j2me-pp-1_0;JavaTextResources"/>
		<rdfs:subClassOf rdf:resource="&java;JavaAPIPart"/>
		<rdfs:seeAlso rdf:resource="&j2se-1_3;JavaUtil"/>
		<rdfs:seeAlso rdf:resource="&j2se-1_3;JavaLang"/>
		<rdfs:comment xml:lang="en">Java API part implementing the java.text.resources package for J2SE 1.3</rdfs:comment>
	</owl:Class>
	<owl:Class rdf:about="&j2se-1_3;JavaAwt">
		<rdfs:subClassOf rdf:resource="&j2me-pp-1_0;JavaAwt"/>
		<rdfs:subClassOf rdf:resource="&j2se-1_2;JavaAwt"/>
		<rdfs:seeAlso rdf:resource="&j2se-1_3;JavaBeans"/>
		<rdfs:seeAlso rdf:resource="&j2se-1_3;JavaAwtImageRenderable"/>
		<rdfs:seeAlso rdf:resource="&j2se-1_3;JavaIo"/>
		<rdfs:seeAlso rdf:resource="&j2se-1_3;JavaAwtEvent"/>
		<rdfs:seeAlso rdf:resource="&j2se-1_3;JavaxSwingText"/>
		<rdfs:seeAlso rdf:resource="&j2se-1_3;JavaUtil"/>
		<rdfs:seeAlso rdf:resource="&j2se-1_3;JavaNet"/>
		<rdfs:seeAlso rdf:resource="&j2se-1_3;JavaAwtColor"/>
		<rdfs:seeAlso rdf:resource="&j2se-1_3;JavaAwtIm"/>
		<rdfs:seeAlso rdf:resource="&j2se-1_3;JavaAwtDnd"/>
		<rdfs:seeAlso rdf:resource="&j2se-1_3;JavaAwtDatatransfer"/>
		<rdfs:seeAlso rdf:resource="&j2se-1_3;JavaSecurity"/>
		<rdfs:seeAlso rdf:resource="&j2se-1_3;JavaAwtImage"/>
		<rdfs:seeAlso rdf:resource="&j2se-1_3;JavaAwtGeom"/>
		<rdfs:seeAlso rdf:resource="&j2se-1_3;JavaText"/>
		<rdfs:seeAlso rdf:resource="&j2se-1_3;JavaLang"/>
		<rdfs:seeAlso rdf:resource="&j2se-1_3;JavaAwtFont"/>
		<rdfs:seeAlso rdf:resource="&j2se-1_3;JavaxAccessibility"/>
		<rdfs:comment xml:lang="en">Java API part implementing the java.awt package for J2SE 1.3</rdfs:comment>
	</owl:Class>
	<owl:Class rdf:about="&j2se-1_3;JavaAwtGeom">
		<rdfs:subClassOf rdf:resource="&j2se-1_2;JavaAwtGeom"/>
		<rdfs:seeAlso rdf:resource="&j2se-1_3;JavaAwt"/>
		<rdfs:seeAlso rdf:resource="&j2se-1_3;JavaLang"/>
		<rdfs:seeAlso rdf:resource="&j2se-1_3;JavaIo"/>
		<rdfs:comment xml:lang="en">Java API part implementing the java.awt.geom package for J2SE 1.3</rdfs:comment>
	</owl:Class>
	<owl:Class rdf:about="&j2se-1_3;JavaAwtEvent">
		<rdfs:subClassOf rdf:resource="&j2me-pp-1_0;JavaAwtEvent"/>
		<rdfs:subClassOf rdf:resource="&j2se-1_2;JavaAwtEvent"/>
		<rdfs:seeAlso rdf:resource="&j2se-1_3;JavaText"/>
		<rdfs:seeAlso rdf:resource="&j2se-1_3;JavaUtil"/>
		<rdfs:seeAlso rdf:resource="&j2se-1_3;JavaAwt"/>
		<rdfs:seeAlso rdf:resource="&j2se-1_3;JavaLang"/>
		<rdfs:seeAlso rdf:resource="&j2se-1_3;JavaAwtFont"/>
		<rdfs:comment xml:lang="en">Java API part implementing the java.awt.event package for J2SE 1.3</rdfs:comment>
	</owl:Class>
	<owl:Class rdf:about="&j2se-1_3;JavaAwtFont">
		<rdfs:subClassOf rdf:resource="&java;JavaAPIPart"/>
		<rdfs:seeAlso rdf:resource="&j2se-1_3;JavaAwtGeom"/>
		<rdfs:seeAlso rdf:resource="&j2se-1_3;JavaIo"/>
		<rdfs:seeAlso rdf:resource="&j2se-1_3;JavaText"/>
		<rdfs:seeAlso rdf:resource="&j2se-1_3;JavaUtil"/>
		<rdfs:seeAlso rdf:resource="&j2se-1_3;JavaAwt"/>
		<rdfs:seeAlso rdf:resource="&j2se-1_3;JavaLang"/>
		<rdfs:comment xml:lang="en">Java API part implementing the java.awt.font package for J2SE 1.3</rdfs:comment>
	</owl:Class>
	<owl:Class rdf:about="&j2se-1_3;JavaAwtImage">
		<rdfs:subClassOf rdf:resource="&j2me-pp-1_0;JavaAwtImage"/>
		<rdfs:subClassOf rdf:resource="&j2se-1_2;JavaAwtImage"/>
		<rdfs:seeAlso rdf:resource="&j2se-1_3;JavaAwtGeom"/>
		<rdfs:seeAlso rdf:resource="&j2se-1_3;JavaMath"/>
		<rdfs:seeAlso rdf:resource="&j2se-1_3;JavaUtil"/>
		<rdfs:seeAlso rdf:resource="&j2se-1_3;JavaAwt"/>
		<rdfs:seeAlso rdf:resource="&j2se-1_3;JavaAwtColor"/>
		<rdfs:seeAlso rdf:resource="&j2se-1_3;JavaLang"/>
		<rdfs:comment xml:lang="en">Java API part implementing the java.awt.image package for J2SE 1.3</rdfs:comment>
	</owl:Class>
	<owl:Class rdf:about="&j2se-1_3;JavaAwtImageRenderable">
		<rdfs:subClassOf rdf:resource="&j2se-1_2;JavaAwtImageRenderable"/>
		<rdfs:seeAlso rdf:resource="&j2se-1_3;JavaAwtGeom"/>
		<rdfs:seeAlso rdf:resource="&j2se-1_3;JavaIo"/>
		<rdfs:seeAlso rdf:resource="&j2se-1_3;JavaUtil"/>
		<rdfs:seeAlso rdf:resource="&j2se-1_3;JavaAwtImage"/>
		<rdfs:seeAlso rdf:resource="&j2se-1_3;JavaAwt"/>
		<rdfs:seeAlso rdf:resource="&j2se-1_3;JavaLang"/>
		<rdfs:comment xml:lang="en">Java API part implementing the java.awt.image.renderable package for J2SE 1.3</rdfs:comment>
	</owl:Class>
	<owl:Class rdf:about="&j2se-1_3;JavaAwtDnd">
		<owl:equivalentClass rdf:resource="&j2se-1_2;JavaAwtDnd"/>
		<rdfs:subClassOf rdf:resource="&java;JavaAPIPart"/>
		<rdfs:seeAlso rdf:resource="&j2se-1_3;JavaIo"/>
		<rdfs:seeAlso rdf:resource="&j2se-1_3;JavaAwtEvent"/>
		<rdfs:seeAlso rdf:resource="&j2se-1_3;JavaUtil"/>
		<rdfs:seeAlso rdf:resource="&j2se-1_3;JavaAwt"/>
		<rdfs:seeAlso rdf:resource="&j2se-1_3;JavaLang"/>
		<rdfs:seeAlso rdf:resource="&j2se-1_3;JavaAwtDatatransfer"/>
		<rdfs:comment xml:lang="en">Java API part implementing the java.awt.dnd package for J2SE 1.3</rdfs:comment>
	</owl:Class>
	<owl:Class rdf:about="&j2se-1_3;JavaAwtIm">
		<rdfs:subClassOf rdf:resource="&j2se-1_2;JavaAwtIm"/>
		<rdfs:seeAlso rdf:resource="&j2se-1_3;JavaText"/>
		<rdfs:seeAlso rdf:resource="&j2se-1_3;JavaUtil"/>
		<rdfs:seeAlso rdf:resource="&j2se-1_3;JavaAwt"/>
		<rdfs:seeAlso rdf:resource="&j2se-1_3;JavaLang"/>
		<rdfs:seeAlso rdf:resource="&j2se-1_3;JavaAwtFont"/>
		<rdfs:comment xml:lang="en">Java API part implementing the java.awt.im package for J2SE 1.3</rdfs:comment>
	</owl:Class>
	<owl:Class rdf:about="&j2se-1_3;JavaAwtImSpi">
		<rdfs:subClassOf rdf:resource="&java;JavaAPIPart"/>
		<rdfs:seeAlso rdf:resource="&j2se-1_3;JavaText"/>
		<rdfs:seeAlso rdf:resource="&j2se-1_3;JavaUtil"/>
		<rdfs:seeAlso rdf:resource="&j2se-1_3;JavaAwt"/>
		<rdfs:seeAlso rdf:resource="&j2se-1_3;JavaLang"/>
		<rdfs:seeAlso rdf:resource="&j2se-1_3;JavaAwtFont"/>
		<rdfs:seeAlso rdf:resource="&j2se-1_3;JavaAwtIm"/>
		<rdfs:comment xml:lang="en">Java API part implementing the java.awt.im.spi package for J2SE 1.3</rdfs:comment>
	</owl:Class>
	<owl:Class rdf:about="&j2se-1_3;JavaAwtColor">
		<rdfs:subClassOf rdf:resource="&j2me-pp-1_0;JavaAwtColor"/>
		<rdfs:subClassOf rdf:resource="&j2se-1_2;JavaAwtColor"/>
		<rdfs:seeAlso rdf:resource="&j2se-1_3;JavaLang"/>
		<rdfs:seeAlso rdf:resource="&j2se-1_3;JavaIo"/>
		<rdfs:comment xml:lang="en">Java API part implementing the java.awt.color package for J2SE 1.3</rdfs:comment>
	</owl:Class>
	<owl:Class rdf:about="&j2se-1_3;JavaAwtDatatransfer">
		<rdfs:subClassOf rdf:resource="&j2me-pp-1_0;JavaAwtDatatransfer"/>
		<rdfs:subClassOf rdf:resource="&j2se-1_2;JavaAwtDatatransfer"/>
		<rdfs:seeAlso rdf:resource="&j2se-1_3;JavaUtil"/>
		<rdfs:seeAlso rdf:resource="&j2se-1_3;JavaLang"/>
		<rdfs:seeAlso rdf:resource="&j2se-1_3;JavaIo"/>
		<rdfs:comment xml:lang="en">Java API part implementing the java.awt.datatransfer package for J2SE 1.3</rdfs:comment>
	</owl:Class>
	<owl:Class rdf:about="&j2se-1_3;JavaAwtPrint">
		<owl:equivalentClass rdf:resource="&j2se-1_2;JavaAwtPrint"/>
		<rdfs:subClassOf rdf:resource="&java;JavaAPIPart"/>
		<rdfs:seeAlso rdf:resource="&j2se-1_3;JavaAwt"/>
		<rdfs:seeAlso rdf:resource="&j2se-1_3;JavaLang"/>
		<rdfs:seeAlso rdf:resource="&j2se-1_3;JavaIo"/>
		<rdfs:comment xml:lang="en">Java API part implementing the java.awt.print package for J2SE 1.3</rdfs:comment>
	</owl:Class>
	<owl:Class rdf:about="&j2se-1_3;JavaBeans">
		<owl:equivalentClass rdf:resource="&j2se-1_2;JavaBeans"/>
		<rdfs:subClassOf rdf:resource="&j2me-pp-1_0;JavaBeans"/>
		<rdfs:seeAlso rdf:resource="&j2se-1_3;JavaLangReflect"/>
		<rdfs:seeAlso rdf:resource="&j2se-1_3;JavaBeansBeancontext"/>
		<rdfs:seeAlso rdf:resource="&j2se-1_3;JavaIo"/>
		<rdfs:seeAlso rdf:resource="&j2se-1_3;JavaUtil"/>
		<rdfs:seeAlso rdf:resource="&j2se-1_3;JavaAwt"/>
		<rdfs:seeAlso rdf:resource="&j2se-1_3;JavaApplet"/>
		<rdfs:seeAlso rdf:resource="&j2se-1_3;JavaLang"/>
		<rdfs:comment xml:lang="en">Java API part implementing the java.beans package for J2SE 1.3</rdfs:comment>
	</owl:Class>
	<owl:Class rdf:about="&j2se-1_3;JavaBeansBeancontext">
		<owl:equivalentClass rdf:resource="&j2se-1_2;JavaBeansBeancontext"/>
		<rdfs:subClassOf rdf:resource="&java;JavaAPIPart"/>
		<rdfs:seeAlso rdf:resource="&j2se-1_3;JavaBeans"/>
		<rdfs:seeAlso rdf:resource="&j2se-1_3;JavaIo"/>
		<rdfs:seeAlso rdf:resource="&j2se-1_3;JavaUtil"/>
		<rdfs:seeAlso rdf:resource="&j2se-1_3;JavaAwt"/>
		<rdfs:seeAlso rdf:resource="&j2se-1_3;JavaNet"/>
		<rdfs:seeAlso rdf:resource="&j2se-1_3;JavaLang"/>
		<rdfs:comment xml:lang="en">Java API part implementing the java.beans.beancontext package for J2SE 1.3</rdfs:comment>
	</owl:Class>
	<owl:Class rdf:about="&j2se-1_3;JavaApplet">
		<rdfs:subClassOf rdf:resource="&j2me-pp-1_0;JavaApplet"/>
		<rdfs:subClassOf rdf:resource="&j2se-1_2;JavaApplet"/>
		<rdfs:seeAlso rdf:resource="&j2se-1_3;JavaxAccessibility"/>
		<rdfs:seeAlso rdf:resource="&j2se-1_3;JavaUtil"/>
		<rdfs:seeAlso rdf:resource="&j2se-1_3;JavaAwt"/>
		<rdfs:seeAlso rdf:resource="&j2se-1_3;JavaNet"/>
		<rdfs:seeAlso rdf:resource="&j2se-1_3;JavaLang"/>
		<rdfs:comment xml:lang="en">Java API part implementing the java.applet package for J2SE 1.3</rdfs:comment>
	</owl:Class>
	<owl:Class rdf:about="&j2se-1_3;JavaRmi">
		<owl:equivalentClass rdf:resource="&j2se-1_2;JavaRmi"/>
		<rdfs:subClassOf rdf:resource="&j2me-pp-1_0;JavaRmi"/>
		<rdfs:seeAlso rdf:resource="&j2se-1_3;JavaLang"/>
		<rdfs:seeAlso rdf:resource="&j2se-1_3;JavaIo"/>
		<rdfs:comment xml:lang="en">Java API part implementing the java.rmi package for J2SE 1.3</rdfs:comment>
	</owl:Class>
	<owl:Class rdf:about="&j2se-1_3;JavaRmiServer">
		<rdfs:subClassOf rdf:resource="&j2se-1_2;JavaRmiServer"/>
		<rdfs:seeAlso rdf:resource="&j2se-1_3;JavaLangReflect"/>
		<rdfs:seeAlso rdf:resource="&j2se-1_3;JavaIo"/>
		<rdfs:seeAlso rdf:resource="&j2se-1_3;JavaRmi"/>
		<rdfs:seeAlso rdf:resource="&j2se-1_3;JavaNet"/>
		<rdfs:seeAlso rdf:resource="&j2se-1_3;JavaLang"/>
		<rdfs:comment xml:lang="en">Java API part implementing the java.rmi.server package for J2SE 1.3</rdfs:comment>
	</owl:Class>
	<owl:Class rdf:about="&j2se-1_3;JavaRmiDgc">
		<owl:equivalentClass rdf:resource="&j2se-1_2;JavaRmiDgc"/>
		<rdfs:subClassOf rdf:resource="&java;JavaAPIPart"/>
		<rdfs:seeAlso rdf:resource="&j2se-1_3;JavaRmi"/>
		<rdfs:seeAlso rdf:resource="&j2se-1_3;JavaLang"/>
		<rdfs:seeAlso rdf:resource="&j2se-1_3;JavaIo"/>
		<rdfs:comment xml:lang="en">Java API part implementing the java.rmi.dgc package for J2SE 1.3</rdfs:comment>
	</owl:Class>
	<owl:Class rdf:about="&j2se-1_3;JavaRmiRegistry">
		<owl:equivalentClass rdf:resource="&j2se-1_2;JavaRmiRegistry"/>
		<rdfs:subClassOf rdf:resource="&j2me-pp-1_0;JavaRmiRegistry"/>
		<rdfs:seeAlso rdf:resource="&j2se-1_3;JavaRmi"/>
		<rdfs:seeAlso rdf:resource="&j2se-1_3;JavaRmiServer"/>
		<rdfs:seeAlso rdf:resource="&j2se-1_3;JavaLang"/>
		<rdfs:comment xml:lang="en">Java API part implementing the java.rmi.registry package for J2SE 1.3</rdfs:comment>
	</owl:Class>
	<owl:Class rdf:about="&j2se-1_3;JavaRmiActivation">
		<owl:equivalentClass rdf:resource="&j2se-1_2;JavaRmiActivation"/>
		<rdfs:subClassOf rdf:resource="&java;JavaAPIPart"/>
		<rdfs:seeAlso rdf:resource="&j2se-1_3;JavaIo"/>
		<rdfs:seeAlso rdf:resource="&j2se-1_3;JavaRmi"/>
		<rdfs:seeAlso rdf:resource="&j2se-1_3;JavaRmiServer"/>
		<rdfs:seeAlso rdf:resource="&j2se-1_3;JavaUtil"/>
		<rdfs:seeAlso rdf:resource="&j2se-1_3;JavaLang"/>
		<rdfs:comment xml:lang="en">Java API part implementing the java.rmi.activation package for J2SE 1.3</rdfs:comment>
	</owl:Class>
	<owl:Class rdf:about="&j2se-1_3;JavaSql">
		<rdfs:subClassOf rdf:resource="&j2se-1_2;JavaSql"/>
		<rdfs:seeAlso rdf:resource="&j2se-1_3;JavaIo"/>
		<rdfs:seeAlso rdf:resource="&j2se-1_3;JavaSecurity"/>
		<rdfs:seeAlso rdf:resource="&j2se-1_3;JavaMath"/>
		<rdfs:seeAlso rdf:resource="&j2se-1_3;JavaUtil"/>
		<rdfs:seeAlso rdf:resource="&j2se-1_3;JavaLang"/>
		<rdfs:comment xml:lang="en">Java API part implementing the java.sql package for J2SE 1.3</rdfs:comment>
	</owl:Class>
	<owl:Class rdf:about="&j2se-1_3;JavaxAccessibility">
		<rdfs:subClassOf rdf:resource="&j2se-1_2;JavaxAccessibility"/>
		<rdfs:seeAlso rdf:resource="&j2se-1_3;JavaBeans"/>
		<rdfs:seeAlso rdf:resource="&j2se-1_3;JavaAwtEvent"/>
		<rdfs:seeAlso rdf:resource="&j2se-1_3;JavaxSwingText"/>
		<rdfs:seeAlso rdf:resource="&j2se-1_3;JavaUtil"/>
		<rdfs:seeAlso rdf:resource="&j2se-1_3;JavaAwt"/>
		<rdfs:seeAlso rdf:resource="&j2se-1_3;JavaLang"/>
		<rdfs:comment xml:lang="en">Java API part implementing the javax.accessibility package for J2SE 1.3</rdfs:comment>
	</owl:Class>
	<owl:Class rdf:about="&j2se-1_3;JavaxSwing">
		<rdfs:subClassOf rdf:resource="&java;JavaAPIPart"/>
		<rdfs:seeAlso rdf:resource="&j2se-1_3;JavaBeans"/>
		<rdfs:seeAlso rdf:resource="&j2se-1_3;JavaIo"/>
		<rdfs:seeAlso rdf:resource="&j2se-1_3;JavaAwtEvent"/>
		<rdfs:seeAlso rdf:resource="&j2se-1_3;JavaApplet"/>
		<rdfs:seeAlso rdf:resource="&j2se-1_3;JavaxSwingTable"/>
		<rdfs:seeAlso rdf:resource="&j2se-1_3;JavaText"/>
		<rdfs:seeAlso rdf:resource="&j2se-1_3;JavaAwt"/>
		<rdfs:seeAlso rdf:resource="&j2se-1_3;JavaxSwingColorchooser"/>
		<rdfs:seeAlso rdf:resource="&j2se-1_3;JavaxAccessibility"/>
		<rdfs:seeAlso rdf:resource="&j2se-1_3;JavaxSwingPlaf"/>
		<rdfs:seeAlso rdf:resource="&j2se-1_3;JavaxSwingText"/>
		<rdfs:seeAlso rdf:resource="&j2se-1_3;JavaUtil"/>
		<rdfs:seeAlso rdf:resource="&j2se-1_3;JavaxSwingTree"/>
		<rdfs:seeAlso rdf:resource="&j2se-1_3;JavaNet"/>
		<rdfs:seeAlso rdf:resource="&j2se-1_3;JavaxSwingBorder"/>
		<rdfs:seeAlso rdf:resource="&j2se-1_3;JavaxSwingEvent"/>
		<rdfs:seeAlso rdf:resource="&j2se-1_3;JavaAwtImage"/>
		<rdfs:seeAlso rdf:resource="&j2se-1_3;JavaLang"/>
		<rdfs:seeAlso rdf:resource="&j2se-1_3;JavaxSwingFilechooser"/>
		<rdfs:comment xml:lang="en">Java API part implementing the javax.swing package for J2SE 1.3</rdfs:comment>
	</owl:Class>
	<owl:Class rdf:about="&j2se-1_3;JavaxSwingText">
		<rdfs:subClassOf rdf:resource="&j2se-1_2;JavaxSwingText"/>
		<rdfs:seeAlso rdf:resource="&j2se-1_3;JavaIo"/>
		<rdfs:seeAlso rdf:resource="&j2se-1_3;JavaAwtEvent"/>
		<rdfs:seeAlso rdf:resource="&j2se-1_3;JavaxSwingPlaf"/>
		<rdfs:seeAlso rdf:resource="&j2se-1_3;JavaUtil"/>
		<rdfs:seeAlso rdf:resource="&j2se-1_3;JavaxSwingTree"/>
		<rdfs:seeAlso rdf:resource="&j2se-1_3;JavaAwtIm"/>
		<rdfs:seeAlso rdf:resource="&j2se-1_3;JavaxSwingEvent"/>
		<rdfs:seeAlso rdf:resource="&j2se-1_3;JavaxSwingPlafBasic"/>
		<rdfs:seeAlso rdf:resource="&j2se-1_3;JavaText"/>
		<rdfs:seeAlso rdf:resource="&j2se-1_3;JavaAwt"/>
		<rdfs:seeAlso rdf:resource="&j2se-1_3;JavaLang"/>
		<rdfs:seeAlso rdf:resource="&j2se-1_3;JavaxSwing"/>
		<rdfs:seeAlso rdf:resource="&j2se-1_3;JavaxSwingUndo"/>
		<rdfs:seeAlso rdf:resource="&j2se-1_3;JavaxAccessibility"/>
		<rdfs:comment xml:lang="en">Java API part implementing the javax.swing.text package for J2SE 1.3</rdfs:comment>
	</owl:Class>
	<owl:Class rdf:about="&j2se-1_3;JavaxSwingTextHtml">
		<rdfs:subClassOf rdf:resource="&j2se-1_2;JavaxSwingTextHtml"/>
		<rdfs:seeAlso rdf:resource="&j2se-1_3;JavaIo"/>
		<rdfs:seeAlso rdf:resource="&j2se-1_3;JavaAwtEvent"/>
		<rdfs:seeAlso rdf:resource="&j2se-1_3;JavaxSwingText"/>
		<rdfs:seeAlso rdf:resource="&j2se-1_3;JavaUtil"/>
		<rdfs:seeAlso rdf:resource="&j2se-1_3;JavaNet"/>
		<rdfs:seeAlso rdf:resource="&j2se-1_3;JavaxSwingEvent"/>
		<rdfs:seeAlso rdf:resource="&j2se-1_3;JavaAwt"/>
		<rdfs:seeAlso rdf:resource="&j2se-1_3;JavaLang"/>
		<rdfs:seeAlso rdf:resource="&j2se-1_3;JavaxSwing"/>
		<rdfs:comment xml:lang="en">Java API part implementing the javax.swing.text.html package for J2SE 1.3</rdfs:comment>
	</owl:Class>
	<owl:Class rdf:about="&j2se-1_3;JavaxSwingTextHtmlParser">
		<rdfs:subClassOf rdf:resource="&j2se-1_2;JavaxSwingTextHtmlParser"/>
		<rdfs:seeAlso rdf:resource="&j2se-1_3;JavaIo"/>
		<rdfs:seeAlso rdf:resource="&j2se-1_3;JavaxSwingTextHtml"/>
		<rdfs:seeAlso rdf:resource="&j2se-1_3;JavaxSwingText"/>
		<rdfs:seeAlso rdf:resource="&j2se-1_3;JavaUtil"/>
		<rdfs:seeAlso rdf:resource="&j2se-1_3;JavaLang"/>
		<rdfs:comment xml:lang="en">Java API part implementing the javax.swing.text.html.parser package for J2SE 1.3</rdfs:comment>
	</owl:Class>
	<owl:Class rdf:about="&j2se-1_3;JavaxSwingTextRtf">
		<owl:equivalentClass rdf:resource="&j2se-1_2;JavaxSwingTextRtf"/>
		<rdfs:subClassOf rdf:resource="&java;JavaAPIPart"/>
		<rdfs:seeAlso rdf:resource="&j2se-1_3;JavaxSwingText"/>
		<rdfs:seeAlso rdf:resource="&j2se-1_3;JavaLang"/>
		<rdfs:seeAlso rdf:resource="&j2se-1_3;JavaIo"/>
		<rdfs:comment xml:lang="en">Java API part implementing the javax.swing.text.rtf package for J2SE 1.3</rdfs:comment>
	</owl:Class>
	<owl:Class rdf:about="&j2se-1_3;JavaxSwingEvent">
		<rdfs:subClassOf rdf:resource="&j2se-1_2;JavaxSwingEvent"/>
		<rdfs:seeAlso rdf:resource="&j2se-1_3;JavaxSwingTable"/>
		<rdfs:seeAlso rdf:resource="&j2se-1_3;JavaBeans"/>
		<rdfs:seeAlso rdf:resource="&j2se-1_3;JavaIo"/>
		<rdfs:seeAlso rdf:resource="&j2se-1_3;JavaAwtEvent"/>
		<rdfs:seeAlso rdf:resource="&j2se-1_3;JavaxSwingText"/>
		<rdfs:seeAlso rdf:resource="&j2se-1_3;JavaUtil"/>
		<rdfs:seeAlso rdf:resource="&j2se-1_3;JavaAwt"/>
		<rdfs:seeAlso rdf:resource="&j2se-1_3;JavaxSwingTree"/>
		<rdfs:seeAlso rdf:resource="&j2se-1_3;JavaNet"/>
		<rdfs:seeAlso rdf:resource="&j2se-1_3;JavaLang"/>
		<rdfs:seeAlso rdf:resource="&j2se-1_3;JavaxSwing"/>
		<rdfs:seeAlso rdf:resource="&j2se-1_3;JavaxSwingUndo"/>
		<rdfs:comment xml:lang="en">Java API part implementing the javax.swing.event package for J2SE 1.3</rdfs:comment>
	</owl:Class>
	<owl:Class rdf:about="&j2se-1_3;JavaxSwingPlaf">
		<rdfs:subClassOf rdf:resource="&j2se-1_2;JavaxSwingPlaf"/>
		<rdfs:seeAlso rdf:resource="&j2se-1_3;JavaIo"/>
		<rdfs:seeAlso rdf:resource="&j2se-1_3;JavaAwtEvent"/>
		<rdfs:seeAlso rdf:resource="&j2se-1_3;JavaxSwingText"/>
		<rdfs:seeAlso rdf:resource="&j2se-1_3;JavaAwt"/>
		<rdfs:seeAlso rdf:resource="&j2se-1_3;JavaxSwingTree"/>
		<rdfs:seeAlso rdf:resource="&j2se-1_3;JavaLang"/>
		<rdfs:seeAlso rdf:resource="&j2se-1_3;JavaxSwingBorder"/>
		<rdfs:seeAlso rdf:resource="&j2se-1_3;JavaxSwingFilechooser"/>
		<rdfs:seeAlso rdf:resource="&j2se-1_3;JavaxSwing"/>
		<rdfs:seeAlso rdf:resource="&j2se-1_3;JavaxAccessibility"/>
		<rdfs:comment xml:lang="en">Java API part implementing the javax.swing.plaf package for J2SE 1.3</rdfs:comment>
	</owl:Class>
	<owl:Class rdf:about="&j2se-1_3;JavaxSwingPlafBasic">
		<rdfs:subClassOf rdf:resource="&j2se-1_2;JavaxSwingPlafBasic"/>
		<rdfs:seeAlso rdf:resource="&j2se-1_3;JavaBeans"/>
		<rdfs:seeAlso rdf:resource="&j2se-1_3;JavaIo"/>
		<rdfs:seeAlso rdf:resource="&j2se-1_3;JavaAwtEvent"/>
		<rdfs:seeAlso rdf:resource="&j2se-1_3;JavaxSwingTable"/>
		<rdfs:seeAlso rdf:resource="&j2se-1_3;JavaAwt"/>
		<rdfs:seeAlso rdf:resource="&j2se-1_3;JavaxAccessibility"/>
		<rdfs:seeAlso rdf:resource="&j2se-1_3;JavaxSwingPlaf"/>
		<rdfs:seeAlso rdf:resource="&j2se-1_3;JavaxSwingText"/>
		<rdfs:seeAlso rdf:resource="&j2se-1_3;JavaUtil"/>
		<rdfs:seeAlso rdf:resource="&j2se-1_3;JavaxSwingTree"/>
		<rdfs:seeAlso rdf:resource="&j2se-1_3;JavaxSwingBorder"/>
		<rdfs:seeAlso rdf:resource="&j2se-1_3;JavaxSwingEvent"/>
		<rdfs:seeAlso rdf:resource="&j2se-1_3;JavaLang"/>
		<rdfs:seeAlso rdf:resource="&j2se-1_3;JavaxSwingFilechooser"/>
		<rdfs:seeAlso rdf:resource="&j2se-1_3;JavaxSwing"/>
		<rdfs:comment xml:lang="en">Java API part implementing the javax.swing.plaf.basic package for J2SE 1.3</rdfs:comment>
	</owl:Class>
	<owl:Class rdf:about="&j2se-1_3;JavaxSwingPlafMetal">
		<rdfs:subClassOf rdf:resource="&j2se-1_2;JavaxSwingPlafMetal"/>
		<rdfs:seeAlso rdf:resource="&j2se-1_3;JavaBeans"/>
		<rdfs:seeAlso rdf:resource="&j2se-1_3;JavaIo"/>
		<rdfs:seeAlso rdf:resource="&j2se-1_3;JavaAwtEvent"/>
		<rdfs:seeAlso rdf:resource="&j2se-1_3;JavaxSwingPlaf"/>
		<rdfs:seeAlso rdf:resource="&j2se-1_3;JavaxSwingTree"/>
		<rdfs:seeAlso rdf:resource="&j2se-1_3;JavaxSwingBorder"/>
		<rdfs:seeAlso rdf:resource="&j2se-1_3;JavaxSwingEvent"/>
		<rdfs:seeAlso rdf:resource="&j2se-1_3;JavaxSwingPlafBasic"/>
		<rdfs:seeAlso rdf:resource="&j2se-1_3;JavaAwt"/>
		<rdfs:seeAlso rdf:resource="&j2se-1_3;JavaLang"/>
		<rdfs:seeAlso rdf:resource="&j2se-1_3;JavaxSwing"/>
		<rdfs:comment xml:lang="en">Java API part implementing the javax.swing.plaf.metal package for J2SE 1.3</rdfs:comment>
	</owl:Class>
	<owl:Class rdf:about="&j2se-1_3;JavaxSwingPlafMulti">
		<rdfs:subClassOf rdf:resource="&j2se-1_2;JavaxSwingPlafMulti"/>
		<rdfs:seeAlso rdf:resource="&j2se-1_3;JavaIo"/>
		<rdfs:seeAlso rdf:resource="&j2se-1_3;JavaxSwingPlaf"/>
		<rdfs:seeAlso rdf:resource="&j2se-1_3;JavaxSwingText"/>
		<rdfs:seeAlso rdf:resource="&j2se-1_3;JavaUtil"/>
		<rdfs:seeAlso rdf:resource="&j2se-1_3;JavaxSwingTree"/>
		<rdfs:seeAlso rdf:resource="&j2se-1_3;JavaAwt"/>
		<rdfs:seeAlso rdf:resource="&j2se-1_3;JavaLang"/>
		<rdfs:seeAlso rdf:resource="&j2se-1_3;JavaxSwingFilechooser"/>
		<rdfs:seeAlso rdf:resource="&j2se-1_3;JavaxSwing"/>
		<rdfs:seeAlso rdf:resource="&j2se-1_3;JavaxAccessibility"/>
		<rdfs:comment xml:lang="en">Java API part implementing the javax.swing.plaf.multi package for J2SE 1.3</rdfs:comment>
	</owl:Class>
	<owl:Class rdf:about="&j2se-1_3;JavaxSwingUndo">
		<owl:equivalentClass rdf:resource="&j2se-1_2;JavaxSwingUndo"/>
		<rdfs:subClassOf rdf:resource="&java;JavaAPIPart"/>
		<rdfs:seeAlso rdf:resource="&j2se-1_3;JavaxSwingEvent"/>
		<rdfs:seeAlso rdf:resource="&j2se-1_3;JavaUtil"/>
		<rdfs:seeAlso rdf:resource="&j2se-1_3;JavaLang"/>
		<rdfs:seeAlso rdf:resource="&j2se-1_3;JavaIo"/>
		<rdfs:comment xml:lang="en">Java API part implementing the javax.swing.undo package for J2SE 1.3</rdfs:comment>
	</owl:Class>
	<owl:Class rdf:about="&j2se-1_3;JavaxSwingTree">
		<rdfs:subClassOf rdf:resource="&j2se-1_2;JavaxSwingTree"/>
		<rdfs:seeAlso rdf:resource="&j2se-1_3;JavaBeans"/>
		<rdfs:seeAlso rdf:resource="&j2se-1_3;JavaIo"/>
		<rdfs:seeAlso rdf:resource="&j2se-1_3;JavaAwtEvent"/>
		<rdfs:seeAlso rdf:resource="&j2se-1_3;JavaUtil"/>
		<rdfs:seeAlso rdf:resource="&j2se-1_3;JavaAwt"/>
		<rdfs:seeAlso rdf:resource="&j2se-1_3;JavaLang"/>
		<rdfs:seeAlso rdf:resource="&j2se-1_3;JavaxSwingBorder"/>
		<rdfs:seeAlso rdf:resource="&j2se-1_3;JavaxSwingEvent"/>
		<rdfs:seeAlso rdf:resource="&j2se-1_3;JavaxSwing"/>
		<rdfs:comment xml:lang="en">Java API part implementing the javax.swing.tree package for J2SE 1.3</rdfs:comment>
	</owl:Class>
	<owl:Class rdf:about="&j2se-1_3;JavaxSwingTable">
		<rdfs:subClassOf rdf:resource="&j2se-1_2;JavaxSwingTable"/>
		<rdfs:seeAlso rdf:resource="&j2se-1_3;JavaBeans"/>
		<rdfs:seeAlso rdf:resource="&j2se-1_3;JavaIo"/>
		<rdfs:seeAlso rdf:resource="&j2se-1_3;JavaAwtEvent"/>
		<rdfs:seeAlso rdf:resource="&j2se-1_3;JavaxSwingPlaf"/>
		<rdfs:seeAlso rdf:resource="&j2se-1_3;JavaUtil"/>
		<rdfs:seeAlso rdf:resource="&j2se-1_3;JavaAwt"/>
		<rdfs:seeAlso rdf:resource="&j2se-1_3;JavaLang"/>
		<rdfs:seeAlso rdf:resource="&j2se-1_3;JavaxSwingBorder"/>
		<rdfs:seeAlso rdf:resource="&j2se-1_3;JavaxSwingEvent"/>
		<rdfs:seeAlso rdf:resource="&j2se-1_3;JavaxSwing"/>
		<rdfs:seeAlso rdf:resource="&j2se-1_3;JavaxAccessibility"/>
		<rdfs:comment xml:lang="en">Java API part implementing the javax.swing.table package for J2SE 1.3</rdfs:comment>
	</owl:Class>
	<owl:Class rdf:about="&j2se-1_3;JavaxSwingBorder">
		<rdfs:subClassOf rdf:resource="&j2se-1_2;JavaxSwingBorder"/>
		<rdfs:seeAlso rdf:resource="&j2se-1_3;JavaAwt"/>
		<rdfs:seeAlso rdf:resource="&j2se-1_3;JavaLang"/>
		<rdfs:seeAlso rdf:resource="&j2se-1_3;JavaxSwing"/>
		<rdfs:seeAlso rdf:resource="&j2se-1_3;JavaIo"/>
		<rdfs:comment xml:lang="en">Java API part implementing the javax.swing.border package for J2SE 1.3</rdfs:comment>
	</owl:Class>
	<owl:Class rdf:about="&j2se-1_3;JavaxSwingColorchooser">
		<rdfs:subClassOf rdf:resource="&j2se-1_2;JavaxSwingColorchooser"/>
		<rdfs:seeAlso rdf:resource="&j2se-1_3;JavaxSwingEvent"/>
		<rdfs:seeAlso rdf:resource="&j2se-1_3;JavaxSwing"/>
		<rdfs:seeAlso rdf:resource="&j2se-1_3;JavaIo"/>
		<rdfs:seeAlso rdf:resource="&j2se-1_3;JavaAwt"/>
		<rdfs:seeAlso rdf:resource="&j2se-1_3;JavaLang"/>
		<rdfs:comment xml:lang="en">Java API part implementing the javax.swing.colorchooser package for J2SE 1.3</rdfs:comment>
	</owl:Class>
	<owl:Class rdf:about="&j2se-1_3;JavaxSwingFilechooser">
		<rdfs:subClassOf rdf:resource="&j2se-1_2;JavaxSwingFilechooser"/>
		<rdfs:seeAlso rdf:resource="&j2se-1_3;JavaxSwing"/>
		<rdfs:seeAlso rdf:resource="&j2se-1_3;JavaLang"/>
		<rdfs:seeAlso rdf:resource="&j2se-1_3;JavaIo"/>
		<rdfs:comment xml:lang="en">Java API part implementing the javax.swing.filechooser package for J2SE 1.3</rdfs:comment>
	</owl:Class>
	<owl:Class rdf:about="&j2se-1_3;JavaxNaming">
		<rdfs:subClassOf rdf:resource="&java;JavaAPIPart"/>
		<rdfs:seeAlso rdf:resource="&j2se-1_3;JavaIo"/>
		<rdfs:seeAlso rdf:resource="&j2se-1_3;JavaUtil"/>
		<rdfs:seeAlso rdf:resource="&j2se-1_3;JavaLang"/>
		<rdfs:comment xml:lang="en">Java API part implementing the javax.naming package for J2SE 1.3</rdfs:comment>
	</owl:Class>
	<owl:Class rdf:about="&j2se-1_3;JavaxNamingDirectory">
		<rdfs:subClassOf rdf:resource="&java;JavaAPIPart"/>
		<rdfs:seeAlso rdf:resource="&j2se-1_3;JavaxNaming"/>
		<rdfs:seeAlso rdf:resource="&j2se-1_3;JavaIo"/>
		<rdfs:seeAlso rdf:resource="&j2se-1_3;JavaUtil"/>
		<rdfs:seeAlso rdf:resource="&j2se-1_3;JavaLang"/>
		<rdfs:comment xml:lang="en">Java API part implementing the javax.naming.directory package for J2SE 1.3</rdfs:comment>
	</owl:Class>
	<owl:Class rdf:about="&j2se-1_3;JavaxNamingEvent">
		<rdfs:subClassOf rdf:resource="&java;JavaAPIPart"/>
		<rdfs:seeAlso rdf:resource="&j2se-1_3;JavaxNamingDirectory"/>
		<rdfs:seeAlso rdf:resource="&j2se-1_3;JavaUtil"/>
		<rdfs:seeAlso rdf:resource="&j2se-1_3;JavaxNaming"/>
		<rdfs:seeAlso rdf:resource="&j2se-1_3;JavaLang"/>
		<rdfs:comment xml:lang="en">Java API part implementing the javax.naming.event package for J2SE 1.3</rdfs:comment>
	</owl:Class>
	<owl:Class rdf:about="&j2se-1_3;JavaxNamingLdap">
		<rdfs:subClassOf rdf:resource="&java;JavaAPIPart"/>
		<rdfs:seeAlso rdf:resource="&j2se-1_3;JavaxNamingDirectory"/>
		<rdfs:seeAlso rdf:resource="&j2se-1_3;JavaxNamingEvent"/>
		<rdfs:seeAlso rdf:resource="&j2se-1_3;JavaUtil"/>
		<rdfs:seeAlso rdf:resource="&j2se-1_3;JavaxNaming"/>
		<rdfs:seeAlso rdf:resource="&j2se-1_3;JavaLang"/>
		<rdfs:seeAlso rdf:resource="&j2se-1_3;JavaIo"/>
		<rdfs:comment xml:lang="en">Java API part implementing the javax.naming.ldap package for J2SE 1.3</rdfs:comment>
	</owl:Class>
	<owl:Class rdf:about="&j2se-1_3;JavaxNamingSpi">
		<rdfs:subClassOf rdf:resource="&java;JavaAPIPart"/>
		<rdfs:seeAlso rdf:resource="&j2se-1_3;JavaxNamingDirectory"/>
		<rdfs:seeAlso rdf:resource="&j2se-1_3;JavaUtil"/>
		<rdfs:seeAlso rdf:resource="&j2se-1_3;JavaxNaming"/>
		<rdfs:seeAlso rdf:resource="&j2se-1_3;JavaLang"/>
		<rdfs:seeAlso rdf:resource="&j2se-1_3;JavaIo"/>
		<rdfs:comment xml:lang="en">Java API part implementing the javax.naming.spi package for J2SE 1.3</rdfs:comment>
	</owl:Class>
	<owl:Class rdf:about="&j2se-1_3;JavaxSoundMidi">
		<rdfs:subClassOf rdf:resource="&java;JavaAPIPart"/>
		<rdfs:seeAlso rdf:resource="&j2se-1_3;JavaUtil"/>
		<rdfs:seeAlso rdf:resource="&j2se-1_3;JavaNet"/>
		<rdfs:seeAlso rdf:resource="&j2se-1_3;JavaLang"/>
		<rdfs:seeAlso rdf:resource="&j2se-1_3;JavaIo"/>
		<rdfs:comment xml:lang="en">Java API part implementing the javax.sound.midi package for J2SE 1.3</rdfs:comment>
	</owl:Class>
	<owl:Class rdf:about="&j2se-1_3;JavaxSoundMidiSpi">
		<rdfs:subClassOf rdf:resource="&java;JavaAPIPart"/>
		<rdfs:seeAlso rdf:resource="&j2se-1_3;JavaNet"/>
		<rdfs:seeAlso rdf:resource="&j2se-1_3;JavaLang"/>
		<rdfs:seeAlso rdf:resource="&j2se-1_3;JavaxSoundMidi"/>
		<rdfs:seeAlso rdf:resource="&j2se-1_3;JavaIo"/>
		<rdfs:comment xml:lang="en">Java API part implementing the javax.sound.midi.spi package for J2SE 1.3</rdfs:comment>
	</owl:Class>
	<owl:Class rdf:about="&j2se-1_3;JavaxSoundSampled">
		<rdfs:subClassOf rdf:resource="&java;JavaAPIPart"/>
		<rdfs:seeAlso rdf:resource="&j2se-1_3;JavaUtil"/>
		<rdfs:seeAlso rdf:resource="&j2se-1_3;JavaNet"/>
		<rdfs:seeAlso rdf:resource="&j2se-1_3;JavaLang"/>
		<rdfs:seeAlso rdf:resource="&j2se-1_3;JavaIo"/>
		<rdfs:seeAlso rdf:resource="&j2se-1_3;JavaSecurity"/>
		<rdfs:comment xml:lang="en">Java API part implementing the javax.sound.sampled package for J2SE 1.3</rdfs:comment>
	</owl:Class>
	<owl:Class rdf:about="&j2se-1_3;JavaxSoundSampledSpi">
		<rdfs:subClassOf rdf:resource="&java;JavaAPIPart"/>
		<rdfs:seeAlso rdf:resource="&j2se-1_3;JavaIo"/>
		<rdfs:seeAlso rdf:resource="&j2se-1_3;JavaNet"/>
		<rdfs:seeAlso rdf:resource="&j2se-1_3;JavaLang"/>
		<rdfs:seeAlso rdf:resource="&j2se-1_3;JavaxSoundSampled"/>
		<rdfs:comment xml:lang="en">Java API part implementing the javax.sound.sampled.spi package for J2SE 1.3</rdfs:comment>
	</owl:Class>
	<owl:Class rdf:about="&j2se-1_3;JavaxRmi">
		<rdfs:subClassOf rdf:resource="&java;JavaAPIPart"/>
		<rdfs:seeAlso rdf:resource="&j2se-1_3;JavaRmi"/>
		<rdfs:seeAlso rdf:resource="&j2se-1_3;JavaLang"/>
		<rdfs:comment xml:lang="en">Java API part implementing the javax.rmi package for J2SE 1.3</rdfs:comment>
	</owl:Class>
	<owl:Class rdf:about="&j2se-1_3;JavaxRmiCORBA">
		<rdfs:subClassOf rdf:resource="&java;JavaAPIPart"/>
		<rdfs:seeAlso rdf:resource="&j2se-1_3;OrgOmgCORBAPortable"/>
		<rdfs:seeAlso rdf:resource="&j2se-1_3;OrgOmgCORBA_2_3Portable"/>
		<rdfs:seeAlso rdf:resource="&j2se-1_3;JavaIo"/>
		<rdfs:seeAlso rdf:resource="&j2se-1_3;OrgOmgSendingContext"/>
		<rdfs:seeAlso rdf:resource="&j2se-1_3;OrgOmgCORBA"/>
		<rdfs:seeAlso rdf:resource="&j2se-1_3;JavaRmi"/>
		<rdfs:seeAlso rdf:resource="&j2se-1_3;JavaLang"/>
		<rdfs:comment xml:lang="en">Java API part implementing the javax.rmi.CORBA package for J2SE 1.3</rdfs:comment>
	</owl:Class>
	<owl:Class rdf:about="&j2se-1_3;JavaxTransaction">
		<rdfs:subClassOf rdf:resource="&java;JavaAPIPart"/>
		<rdfs:seeAlso rdf:resource="&j2se-1_3;JavaRmi"/>
		<rdfs:seeAlso rdf:resource="&j2se-1_3;JavaLang"/>
		<rdfs:comment xml:lang="en">Java API part implementing the javax.transaction package for J2SE 1.3</rdfs:comment>
	</owl:Class>
	<owl:Class rdf:about="&j2se-1_3;OrgOmgCORBA_2_3">
		<rdfs:subClassOf rdf:resource="&java;JavaAPIPart"/>
		<rdfs:seeAlso rdf:resource="&j2se-1_3;OrgOmgCORBAPortable"/>
		<rdfs:seeAlso rdf:resource="&j2se-1_3;JavaLang"/>
		<rdfs:seeAlso rdf:resource="&j2se-1_3;OrgOmgCORBA"/>
		<rdfs:comment xml:lang="en">Java API part implementing the org.omg.CORBA_2_3 package for J2SE 1.3</rdfs:comment>
	</owl:Class>
	<owl:Class rdf:about="&j2se-1_3;OrgOmgCORBA_2_3Portable">
		<rdfs:subClassOf rdf:resource="&java;JavaAPIPart"/>
		<rdfs:seeAlso rdf:resource="&j2se-1_3;OrgOmgCORBAPortable"/>
		<rdfs:seeAlso rdf:resource="&j2se-1_3;JavaLang"/>
		<rdfs:seeAlso rdf:resource="&j2se-1_3;JavaIo"/>
		<rdfs:seeAlso rdf:resource="&j2se-1_3;OrgOmgCORBA"/>
		<rdfs:comment xml:lang="en">Java API part implementing the org.omg.CORBA_2_3.portable package for J2SE 1.3</rdfs:comment>
	</owl:Class>
	<owl:Class rdf:about="&j2se-1_3;OrgOmgCORBA">
		<rdfs:subClassOf rdf:resource="&j2se-1_2;OrgOmgCORBA"/>
		<rdfs:seeAlso rdf:resource="&j2se-1_3;OrgOmgCORBAPortable"/>
		<rdfs:seeAlso rdf:resource="&j2se-1_3;JavaIo"/>
		<rdfs:seeAlso rdf:resource="&j2se-1_3;JavaMath"/>
		<rdfs:seeAlso rdf:resource="&j2se-1_3;JavaUtil"/>
		<rdfs:seeAlso rdf:resource="&j2se-1_3;JavaApplet"/>
		<rdfs:seeAlso rdf:resource="&j2se-1_3;JavaLang"/>
		<rdfs:comment xml:lang="en">Java API part implementing the org.omg.CORBA package for J2SE 1.3</rdfs:comment>
	</owl:Class>
	<owl:Class rdf:about="&j2se-1_3;OrgOmgCORBAPortable">
		<rdfs:subClassOf rdf:resource="&j2se-1_2;OrgOmgCORBAPortable"/>
		<rdfs:seeAlso rdf:resource="&j2se-1_3;JavaIo"/>
		<rdfs:seeAlso rdf:resource="&j2se-1_3;JavaLang"/>
		<rdfs:seeAlso rdf:resource="&j2se-1_3;OrgOmgCORBA_2_3Portable"/>
		<rdfs:seeAlso rdf:resource="&j2se-1_3;OrgOmgCORBA"/>
		<rdfs:seeAlso rdf:resource="&j2se-1_3;JavaMath"/>
		<rdfs:comment xml:lang="en">Java API part implementing the org.omg.CORBA.portable package for J2SE 1.3</rdfs:comment>
	</owl:Class>
	<owl:Class rdf:about="&j2se-1_3;OrgOmgCORBATypeCodePackage">
		<owl:equivalentClass rdf:resource="&j2se-1_2;OrgOmgCORBATypeCodePackage"/>
		<rdfs:subClassOf rdf:resource="&java;JavaAPIPart"/>
		<rdfs:seeAlso rdf:resource="&j2se-1_3;JavaLang"/>
		<rdfs:seeAlso rdf:resource="&j2se-1_3;OrgOmgCORBA"/>
		<rdfs:comment xml:lang="en">Java API part implementing the org.omg.CORBA.TypeCodePackage package for J2SE 1.3</rdfs:comment>
	</owl:Class>
	<owl:Class rdf:about="&j2se-1_3;OrgOmgCORBAORBPackage">
		<owl:equivalentClass rdf:resource="&j2se-1_2;OrgOmgCORBAORBPackage"/>
		<rdfs:subClassOf rdf:resource="&java;JavaAPIPart"/>
		<rdfs:seeAlso rdf:resource="&j2se-1_3;JavaLang"/>
		<rdfs:seeAlso rdf:resource="&j2se-1_3;OrgOmgCORBA"/>
		<rdfs:comment xml:lang="en">Java API part implementing the org.omg.CORBA.ORBPackage package for J2SE 1.3</rdfs:comment>
	</owl:Class>
	<owl:Class rdf:about="&j2se-1_3;OrgOmgCORBADynAnyPackage">
		<owl:equivalentClass rdf:resource="&j2se-1_2;OrgOmgCORBADynAnyPackage"/>
		<rdfs:subClassOf rdf:resource="&java;JavaAPIPart"/>
		<rdfs:seeAlso rdf:resource="&j2se-1_3;JavaLang"/>
		<rdfs:seeAlso rdf:resource="&j2se-1_3;OrgOmgCORBA"/>
		<rdfs:comment xml:lang="en">Java API part implementing the org.omg.CORBA.DynAnyPackage package for J2SE 1.3</rdfs:comment>
	</owl:Class>
	<owl:Class rdf:about="&j2se-1_3;OrgOmgSendingContext">
		<rdfs:subClassOf rdf:resource="&java;JavaAPIPart"/>
		<rdfs:seeAlso rdf:resource="&j2se-1_3;OrgOmgCORBAPortable"/>
		<rdfs:seeAlso rdf:resource="&j2se-1_3;OrgOmgCORBA"/>
		<rdfs:comment xml:lang="en">Java API part implementing the org.omg.SendingContext package for J2SE 1.3</rdfs:comment>
	</owl:Class>
	<owl:Class rdf:about="&j2se-1_3;OrgOmgCosNaming">
		<rdfs:subClassOf rdf:resource="&j2se-1_2;OrgOmgCosNaming"/>
		<rdfs:seeAlso rdf:resource="&j2se-1_3;OrgOmgCORBAPortable"/>
		<rdfs:seeAlso rdf:resource="&j2se-1_3;OrgOmgCORBA"/>
		<rdfs:seeAlso rdf:resource="&j2se-1_3;JavaLang"/>
		<rdfs:comment xml:lang="en">Java API part implementing the org.omg.CosNaming package for J2SE 1.3</rdfs:comment>
	</owl:Class>
	<owl:Class rdf:about="&j2se-1_3;OrgOmgCosNamingNamingContextPackage">
		<owl:equivalentClass rdf:resource="&j2se-1_2;OrgOmgCosNamingNamingContextPackage"/>
		<rdfs:subClassOf rdf:resource="&java;JavaAPIPart"/>
		<rdfs:seeAlso rdf:resource="&j2se-1_3;OrgOmgCORBAPortable"/>
		<rdfs:seeAlso rdf:resource="&j2se-1_3;OrgOmgCosNaming"/>
		<rdfs:seeAlso rdf:resource="&j2se-1_3;JavaLang"/>
		<rdfs:seeAlso rdf:resource="&j2se-1_3;OrgOmgCORBA"/>
		<rdfs:comment xml:lang="en">Java API part implementing the org.omg.CosNaming.NamingContextPackage package for J2SE 1.3</rdfs:comment>
	</owl:Class>
	<owl:Class rdf:about="&j2se-1_3;OrgOmgStubJavaRmi">
		<rdfs:subClassOf rdf:resource="&java;JavaAPIPart"/>
		<rdfs:seeAlso rdf:resource="&j2se-1_3;JavaRmi"/>
		<rdfs:seeAlso rdf:resource="&j2se-1_3;JavaxRmiCORBA"/>
		<rdfs:comment xml:lang="en">Java API part implementing the org.omg.stub.java.rmi package for J2SE 1.3</rdfs:comment>
	</owl:Class>
	<owl:Class rdf:about="&j2se-1_3;JavaIoAPI">
		<rdfs:subClassOf rdf:resource="&j2me-pp-1_0;JavaIoAPI"/>
		<rdfs:subClassOf rdf:resource="&j2se-1_2;JavaIoAPI"/>
		<rdfs:comment xml:lang="en">JavaLibrary implementing the java.io package for J2SE 1.3</rdfs:comment>
		<rdfs:comment xml:lang="OWLManchester">platform:comprisesInterfacePart some JavaIo</rdfs:comment>
	</owl:Class>
	<owl:Class rdf:about="&j2se-1_3;JavaLangAPI">
		<rdfs:subClassOf rdf:resource="&j2me-pp-1_0;JavaLangAPI"/>
		<rdfs:subClassOf rdf:resource="&j2se-1_2;JavaLangAPI"/>
		<rdfs:comment xml:lang="en">JavaLibrary implementing the java.lang package for J2SE 1.3</rdfs:comment>
		<rdfs:comment xml:lang="OWLManchester">platform:comprisesInterfacePart some JavaLang</rdfs:comment>
	</owl:Class>
	<owl:Class rdf:about="&j2se-1_3;JavaLangReflectAPI">
		<owl:equivalentClass rdf:resource="&j2me-pp-1_0;JavaLangReflectAPI"/>
		<rdfs:subClassOf rdf:resource="&j2se-1_2;JavaLangReflectAPI"/>
		<rdfs:comment xml:lang="en">JavaLibrary implementing the java.lang.reflect package for J2SE 1.3</rdfs:comment>
		<rdfs:comment xml:lang="OWLManchester">platform:comprisesInterfacePart some JavaLangReflect</rdfs:comment>
	</owl:Class>
	<owl:Class rdf:about="&j2se-1_3;JavaLangRefAPI">
		<owl:equivalentClass rdf:resource="&j2me-pp-1_0;JavaLangRefAPI"/>
		<owl:equivalentClass rdf:resource="&j2se-1_2;JavaLangRefAPI"/>
		<rdfs:subClassOf rdf:resource="&java;JavaAPI"/>
		<rdfs:comment xml:lang="en">JavaLibrary implementing the java.lang.ref package for J2SE 1.3</rdfs:comment>
		<rdfs:comment xml:lang="OWLManchester">platform:comprisesInterfacePart some JavaLangRef</rdfs:comment>
	</owl:Class>
	<owl:Class rdf:about="&j2se-1_3;JavaNetAPI">
		<rdfs:subClassOf rdf:resource="&j2me-pp-1_0;JavaNetAPI"/>
		<rdfs:subClassOf rdf:resource="&j2se-1_2;JavaNetAPI"/>
		<rdfs:comment xml:lang="en">JavaLibrary implementing the java.net package for J2SE 1.3</rdfs:comment>
		<rdfs:comment xml:lang="OWLManchester">platform:comprisesInterfacePart some JavaNet</rdfs:comment>
	</owl:Class>
	<owl:Class rdf:about="&j2se-1_3;JavaSecurityAPI">
		<rdfs:subClassOf rdf:resource="&j2me-pp-1_0;JavaSecurityAPI"/>
		<rdfs:subClassOf rdf:resource="&j2se-1_2;JavaSecurityAPI"/>
		<rdfs:comment xml:lang="en">JavaLibrary implementing the java.security package for J2SE 1.3</rdfs:comment>
		<rdfs:comment xml:lang="OWLManchester">platform:comprisesInterfacePart some JavaSecurity</rdfs:comment>
	</owl:Class>
	<owl:Class rdf:about="&j2se-1_3;JavaSecurityCertAPI">
		<owl:equivalentClass rdf:resource="&j2me-pp-1_0;JavaSecurityCertAPI"/>
		<rdfs:subClassOf rdf:resource="&j2se-1_2;JavaSecurityCertAPI"/>
		<rdfs:comment xml:lang="en">JavaLibrary implementing the java.security.cert package for J2SE 1.3</rdfs:comment>
		<rdfs:comment xml:lang="OWLManchester">platform:comprisesInterfacePart some JavaSecurityCert</rdfs:comment>
	</owl:Class>
	<owl:Class rdf:about="&j2se-1_3;JavaSecuritySpecAPI">
		<owl:equivalentClass rdf:resource="&j2me-pp-1_0;JavaSecuritySpecAPI"/>
		<rdfs:subClassOf rdf:resource="&j2se-1_2;JavaSecuritySpecAPI"/>
		<rdfs:comment xml:lang="en">JavaLibrary implementing the java.security.spec package for J2SE 1.3</rdfs:comment>
		<rdfs:comment xml:lang="OWLManchester">platform:comprisesInterfacePart some JavaSecuritySpec</rdfs:comment>
	</owl:Class>
	<owl:Class rdf:about="&j2se-1_3;JavaSecurityInterfacesAPI">
		<owl:equivalentClass rdf:resource="&j2me-pp-1_0;JavaSecurityInterfacesAPI"/>
		<rdfs:subClassOf rdf:resource="&j2se-1_2;JavaSecurityInterfacesAPI"/>
		<rdfs:comment xml:lang="en">JavaLibrary implementing the java.security.interfaces package for J2SE 1.3</rdfs:comment>
		<rdfs:comment xml:lang="OWLManchester">platform:comprisesInterfacePart some JavaSecurityInterfaces</rdfs:comment>
	</owl:Class>
	<owl:Class rdf:about="&j2se-1_3;JavaSecurityAclAPI">
		<owl:equivalentClass rdf:resource="&j2me-pp-1_0;JavaSecurityAclAPI"/>
		<owl:equivalentClass rdf:resource="&j2se-1_2;JavaSecurityAclAPI"/>
		<rdfs:subClassOf rdf:resource="&java;JavaAPI"/>
		<rdfs:comment xml:lang="en">JavaLibrary implementing the java.security.acl package for J2SE 1.3</rdfs:comment>
		<rdfs:comment xml:lang="OWLManchester">platform:comprisesInterfacePart some JavaSecurityAcl</rdfs:comment>
	</owl:Class>
	<owl:Class rdf:about="&j2se-1_3;JavaUtilAPI">
		<rdfs:subClassOf rdf:resource="&j2me-pp-1_0;JavaUtilAPI"/>
		<rdfs:subClassOf rdf:resource="&j2se-1_2;JavaUtilAPI"/>
		<rdfs:comment xml:lang="en">JavaLibrary implementing the java.util package for J2SE 1.3</rdfs:comment>
		<rdfs:comment xml:lang="OWLManchester">platform:comprisesInterfacePart some JavaUtil</rdfs:comment>
	</owl:Class>
	<owl:Class rdf:about="&j2se-1_3;JavaUtilJarAPI">
		<owl:equivalentClass rdf:resource="&j2me-pp-1_0;JavaUtilJarAPI"/>
		<rdfs:subClassOf rdf:resource="&j2se-1_2;JavaUtilJarAPI"/>
		<rdfs:comment xml:lang="en">JavaLibrary implementing the java.util.jar package for J2SE 1.3</rdfs:comment>
		<rdfs:comment xml:lang="OWLManchester">platform:comprisesInterfacePart some JavaUtilJar</rdfs:comment>
	</owl:Class>
	<owl:Class rdf:about="&j2se-1_3;JavaUtilZipAPI">
		<owl:equivalentClass rdf:resource="&j2me-pp-1_0;JavaUtilZipAPI"/>
		<rdfs:subClassOf rdf:resource="&j2se-1_2;JavaUtilZipAPI"/>
		<rdfs:comment xml:lang="en">JavaLibrary implementing the java.util.zip package for J2SE 1.3</rdfs:comment>
		<rdfs:comment xml:lang="OWLManchester">platform:comprisesInterfacePart some JavaUtilZip</rdfs:comment>
	</owl:Class>
	<owl:Class rdf:about="&j2se-1_3;JavaMathAPI">
		<owl:equivalentClass rdf:resource="&j2me-pp-1_0;JavaMathAPI"/>
		<owl:equivalentClass rdf:resource="&j2se-1_2;JavaMathAPI"/>
		<rdfs:subClassOf rdf:resource="&java;JavaAPI"/>
		<rdfs:comment xml:lang="en">JavaLibrary implementing the java.math package for J2SE 1.3</rdfs:comment>
		<rdfs:comment xml:lang="OWLManchester">platform:comprisesInterfacePart some JavaMath</rdfs:comment>
	</owl:Class>
	<owl:Class rdf:about="&j2se-1_3;JavaTextAPI">
		<owl:equivalentClass rdf:resource="&j2me-pp-1_0;JavaTextAPI"/>
		<rdfs:subClassOf rdf:resource="&java;JavaAPI"/>
		<rdfs:comment xml:lang="en">JavaLibrary implementing the java.text package for J2SE 1.3</rdfs:comment>
		<rdfs:comment xml:lang="OWLManchester">platform:comprisesInterfacePart some JavaText</rdfs:comment>
	</owl:Class>
	<owl:Class rdf:about="&j2se-1_3;JavaTextResourcesAPI">
		<owl:equivalentClass rdf:resource="&j2me-pp-1_0;JavaTextResourcesAPI"/>
		<rdfs:subClassOf rdf:resource="&java;JavaAPI"/>
		<rdfs:comment xml:lang="en">JavaLibrary implementing the java.text.resources package for J2SE 1.3</rdfs:comment>
		<rdfs:comment xml:lang="OWLManchester">platform:comprisesInterfacePart some JavaTextResources</rdfs:comment>
	</owl:Class>
	<owl:Class rdf:about="&j2se-1_3;JavaAwtAPI">
		<rdfs:subClassOf rdf:resource="&j2me-pp-1_0;JavaAwtAPI"/>
		<rdfs:subClassOf rdf:resource="&j2se-1_2;JavaAwtAPI"/>
		<rdfs:comment xml:lang="en">JavaLibrary implementing the java.awt package for J2SE 1.3</rdfs:comment>
		<rdfs:comment xml:lang="OWLManchester">platform:comprisesInterfacePart some JavaAwt</rdfs:comment>
	</owl:Class>
	<owl:Class rdf:about="&j2se-1_3;JavaAwtGeomAPI">
		<rdfs:subClassOf rdf:resource="&j2se-1_2;JavaAwtGeomAPI"/>
		<rdfs:comment xml:lang="en">JavaLibrary implementing the java.awt.geom package for J2SE 1.3</rdfs:comment>
		<rdfs:comment xml:lang="OWLManchester">platform:comprisesInterfacePart some JavaAwtGeom</rdfs:comment>
	</owl:Class>
	<owl:Class rdf:about="&j2se-1_3;JavaAwtEventAPI">
		<rdfs:subClassOf rdf:resource="&j2me-pp-1_0;JavaAwtEventAPI"/>
		<rdfs:subClassOf rdf:resource="&j2se-1_2;JavaAwtEventAPI"/>
		<rdfs:comment xml:lang="en">JavaLibrary implementing the java.awt.event package for J2SE 1.3</rdfs:comment>
		<rdfs:comment xml:lang="OWLManchester">platform:comprisesInterfacePart some JavaAwtEvent</rdfs:comment>
	</owl:Class>
	<owl:Class rdf:about="&j2se-1_3;JavaAwtFontAPI">
		<rdfs:subClassOf rdf:resource="&java;JavaAPI"/>
		<rdfs:comment xml:lang="en">JavaLibrary implementing the java.awt.font package for J2SE 1.3</rdfs:comment>
		<rdfs:comment xml:lang="OWLManchester">platform:comprisesInterfacePart some JavaAwtFont</rdfs:comment>
	</owl:Class>
	<owl:Class rdf:about="&j2se-1_3;JavaAwtImageAPI">
		<rdfs:subClassOf rdf:resource="&j2me-pp-1_0;JavaAwtImageAPI"/>
		<rdfs:subClassOf rdf:resource="&j2se-1_2;JavaAwtImageAPI"/>
		<rdfs:comment xml:lang="en">JavaLibrary implementing the java.awt.image package for J2SE 1.3</rdfs:comment>
		<rdfs:comment xml:lang="OWLManchester">platform:comprisesInterfacePart some JavaAwtImage</rdfs:comment>
	</owl:Class>
	<owl:Class rdf:about="&j2se-1_3;JavaAwtImageRenderableAPI">
		<rdfs:subClassOf rdf:resource="&j2se-1_2;JavaAwtImageRenderableAPI"/>
		<rdfs:comment xml:lang="en">JavaLibrary implementing the java.awt.image.renderable package for J2SE 1.3</rdfs:comment>
		<rdfs:comment xml:lang="OWLManchester">platform:comprisesInterfacePart some JavaAwtImageRenderable</rdfs:comment>
	</owl:Class>
	<owl:Class rdf:about="&j2se-1_3;JavaAwtDndAPI">
		<owl:equivalentClass rdf:resource="&j2se-1_2;JavaAwtDndAPI"/>
		<rdfs:subClassOf rdf:resource="&java;JavaAPI"/>
		<rdfs:comment xml:lang="en">JavaLibrary implementing the java.awt.dnd package for J2SE 1.3</rdfs:comment>
		<rdfs:comment xml:lang="OWLManchester">platform:comprisesInterfacePart some JavaAwtDnd</rdfs:comment>
	</owl:Class>
	<owl:Class rdf:about="&j2se-1_3;JavaAwtImAPI">
		<rdfs:subClassOf rdf:resource="&j2se-1_2;JavaAwtImAPI"/>
		<rdfs:comment xml:lang="en">JavaLibrary implementing the java.awt.im package for J2SE 1.3</rdfs:comment>
		<rdfs:comment xml:lang="OWLManchester">platform:comprisesInterfacePart some JavaAwtIm</rdfs:comment>
	</owl:Class>
	<owl:Class rdf:about="&j2se-1_3;JavaAwtImSpiAPI">
		<rdfs:subClassOf rdf:resource="&java;JavaAPI"/>
		<rdfs:comment xml:lang="en">JavaLibrary implementing the java.awt.im.spi package for J2SE 1.3</rdfs:comment>
		<rdfs:comment xml:lang="OWLManchester">platform:comprisesInterfacePart some JavaAwtImSpi</rdfs:comment>
	</owl:Class>
	<owl:Class rdf:about="&j2se-1_3;JavaAwtColorAPI">
		<rdfs:subClassOf rdf:resource="&j2me-pp-1_0;JavaAwtColorAPI"/>
		<rdfs:subClassOf rdf:resource="&j2se-1_2;JavaAwtColorAPI"/>
		<rdfs:comment xml:lang="en">JavaLibrary implementing the java.awt.color package for J2SE 1.3</rdfs:comment>
		<rdfs:comment xml:lang="OWLManchester">platform:comprisesInterfacePart some JavaAwtColor</rdfs:comment>
	</owl:Class>
	<owl:Class rdf:about="&j2se-1_3;JavaAwtDatatransferAPI">
		<rdfs:subClassOf rdf:resource="&j2me-pp-1_0;JavaAwtDatatransferAPI"/>
		<rdfs:subClassOf rdf:resource="&j2se-1_2;JavaAwtDatatransferAPI"/>
		<rdfs:comment xml:lang="en">JavaLibrary implementing the java.awt.datatransfer package for J2SE 1.3</rdfs:comment>
		<rdfs:comment xml:lang="OWLManchester">platform:comprisesInterfacePart some JavaAwtDatatransfer</rdfs:comment>
	</owl:Class>
	<owl:Class rdf:about="&j2se-1_3;JavaAwtPrintAPI">
		<owl:equivalentClass rdf:resource="&j2se-1_2;JavaAwtPrintAPI"/>
		<rdfs:subClassOf rdf:resource="&java;JavaAPI"/>
		<rdfs:comment xml:lang="en">JavaLibrary implementing the java.awt.print package for J2SE 1.3</rdfs:comment>
		<rdfs:comment xml:lang="OWLManchester">platform:comprisesInterfacePart some JavaAwtPrint</rdfs:comment>
	</owl:Class>
	<owl:Class rdf:about="&j2se-1_3;JavaBeansAPI">
		<owl:equivalentClass rdf:resource="&j2se-1_2;JavaBeansAPI"/>
		<rdfs:subClassOf rdf:resource="&j2me-pp-1_0;JavaBeansAPI"/>
		<rdfs:comment xml:lang="en">JavaLibrary implementing the java.beans package for J2SE 1.3</rdfs:comment>
		<rdfs:comment xml:lang="OWLManchester">platform:comprisesInterfacePart some JavaBeans</rdfs:comment>
	</owl:Class>
	<owl:Class rdf:about="&j2se-1_3;JavaBeansBeancontextAPI">
		<owl:equivalentClass rdf:resource="&j2se-1_2;JavaBeansBeancontextAPI"/>
		<rdfs:subClassOf rdf:resource="&java;JavaAPI"/>
		<rdfs:comment xml:lang="en">JavaLibrary implementing the java.beans.beancontext package for J2SE 1.3</rdfs:comment>
		<rdfs:comment xml:lang="OWLManchester">platform:comprisesInterfacePart some JavaBeansBeancontext</rdfs:comment>
	</owl:Class>
	<owl:Class rdf:about="&j2se-1_3;JavaAppletAPI">
		<rdfs:subClassOf rdf:resource="&j2me-pp-1_0;JavaAppletAPI"/>
		<rdfs:subClassOf rdf:resource="&j2se-1_2;JavaAppletAPI"/>
		<rdfs:comment xml:lang="en">JavaLibrary implementing the java.applet package for J2SE 1.3</rdfs:comment>
		<rdfs:comment xml:lang="OWLManchester">platform:comprisesInterfacePart some JavaApplet</rdfs:comment>
	</owl:Class>
	<owl:Class rdf:about="&j2se-1_3;JavaRmiAPI">
		<owl:equivalentClass rdf:resource="&j2se-1_2;JavaRmiAPI"/>
		<rdfs:subClassOf rdf:resource="&j2me-pp-1_0;JavaRmiAPI"/>
		<rdfs:comment xml:lang="en">JavaLibrary implementing the java.rmi package for J2SE 1.3</rdfs:comment>
		<rdfs:comment xml:lang="OWLManchester">platform:comprisesInterfacePart some JavaRmi</rdfs:comment>
	</owl:Class>
	<owl:Class rdf:about="&j2se-1_3;JavaRmiServerAPI">
		<rdfs:subClassOf rdf:resource="&j2se-1_2;JavaRmiServerAPI"/>
		<rdfs:comment xml:lang="en">JavaLibrary implementing the java.rmi.server package for J2SE 1.3</rdfs:comment>
		<rdfs:comment xml:lang="OWLManchester">platform:comprisesInterfacePart some JavaRmiServer</rdfs:comment>
	</owl:Class>
	<owl:Class rdf:about="&j2se-1_3;JavaRmiDgcAPI">
		<owl:equivalentClass rdf:resource="&j2se-1_2;JavaRmiDgcAPI"/>
		<rdfs:subClassOf rdf:resource="&java;JavaAPI"/>
		<rdfs:comment xml:lang="en">JavaLibrary implementing the java.rmi.dgc package for J2SE 1.3</rdfs:comment>
		<rdfs:comment xml:lang="OWLManchester">platform:comprisesInterfacePart some JavaRmiDgc</rdfs:comment>
	</owl:Class>
	<owl:Class rdf:about="&j2se-1_3;JavaRmiRegistryAPI">
		<owl:equivalentClass rdf:resource="&j2se-1_2;JavaRmiRegistryAPI"/>
		<rdfs:subClassOf rdf:resource="&j2me-pp-1_0;JavaRmiRegistryAPI"/>
		<rdfs:comment xml:lang="en">JavaLibrary implementing the java.rmi.registry package for J2SE 1.3</rdfs:comment>
		<rdfs:comment xml:lang="OWLManchester">platform:comprisesInterfacePart some JavaRmiRegistry</rdfs:comment>
	</owl:Class>
	<owl:Class rdf:about="&j2se-1_3;JavaRmiActivationAPI">
		<owl:equivalentClass rdf:resource="&j2se-1_2;JavaRmiActivationAPI"/>
		<rdfs:subClassOf rdf:resource="&java;JavaAPI"/>
		<rdfs:comment xml:lang="en">JavaLibrary implementing the java.rmi.activation package for J2SE 1.3</rdfs:comment>
		<rdfs:comment xml:lang="OWLManchester">platform:comprisesInterfacePart some JavaRmiActivation</rdfs:comment>
	</owl:Class>
	<owl:Class rdf:about="&j2se-1_3;JavaSqlAPI">
		<rdfs:subClassOf rdf:resource="&j2se-1_2;JavaSqlAPI"/>
		<rdfs:comment xml:lang="en">JavaLibrary implementing the java.sql package for J2SE 1.3</rdfs:comment>
		<rdfs:comment xml:lang="OWLManchester">platform:comprisesInterfacePart some JavaSql</rdfs:comment>
	</owl:Class>
	<owl:Class rdf:about="&j2se-1_3;JavaxAccessibilityAPI">
		<rdfs:subClassOf rdf:resource="&j2se-1_2;JavaxAccessibilityAPI"/>
		<rdfs:comment xml:lang="en">JavaLibrary implementing the javax.accessibility package for J2SE 1.3</rdfs:comment>
		<rdfs:comment xml:lang="OWLManchester">platform:comprisesInterfacePart some JavaxAccessibility</rdfs:comment>
	</owl:Class>
	<owl:Class rdf:about="&j2se-1_3;JavaxSwingAPI">
		<rdfs:subClassOf rdf:resource="&java;JavaAPI"/>
		<rdfs:comment xml:lang="en">JavaLibrary implementing the javax.swing package for J2SE 1.3</rdfs:comment>
		<rdfs:comment xml:lang="OWLManchester">platform:comprisesInterfacePart some JavaxSwing</rdfs:comment>
	</owl:Class>
	<owl:Class rdf:about="&j2se-1_3;JavaxSwingTextAPI">
		<rdfs:subClassOf rdf:resource="&j2se-1_2;JavaxSwingTextAPI"/>
		<rdfs:comment xml:lang="en">JavaLibrary implementing the javax.swing.text package for J2SE 1.3</rdfs:comment>
		<rdfs:comment xml:lang="OWLManchester">platform:comprisesInterfacePart some JavaxSwingText</rdfs:comment>
	</owl:Class>
	<owl:Class rdf:about="&j2se-1_3;JavaxSwingTextHtmlAPI">
		<rdfs:subClassOf rdf:resource="&j2se-1_2;JavaxSwingTextHtmlAPI"/>
		<rdfs:comment xml:lang="en">JavaLibrary implementing the javax.swing.text.html package for J2SE 1.3</rdfs:comment>
		<rdfs:comment xml:lang="OWLManchester">platform:comprisesInterfacePart some JavaxSwingTextHtml</rdfs:comment>
	</owl:Class>
	<owl:Class rdf:about="&j2se-1_3;JavaxSwingTextHtmlParserAPI">
		<rdfs:subClassOf rdf:resource="&j2se-1_2;JavaxSwingTextHtmlParserAPI"/>
		<rdfs:comment xml:lang="en">JavaLibrary implementing the javax.swing.text.html.parser package for J2SE 1.3</rdfs:comment>
		<rdfs:comment xml:lang="OWLManchester">platform:comprisesInterfacePart some JavaxSwingTextHtmlParser</rdfs:comment>
	</owl:Class>
	<owl:Class rdf:about="&j2se-1_3;JavaxSwingTextRtfAPI">
		<owl:equivalentClass rdf:resource="&j2se-1_2;JavaxSwingTextRtfAPI"/>
		<rdfs:subClassOf rdf:resource="&java;JavaAPI"/>
		<rdfs:comment xml:lang="en">JavaLibrary implementing the javax.swing.text.rtf package for J2SE 1.3</rdfs:comment>
		<rdfs:comment xml:lang="OWLManchester">platform:comprisesInterfacePart some JavaxSwingTextRtf</rdfs:comment>
	</owl:Class>
	<owl:Class rdf:about="&j2se-1_3;JavaxSwingEventAPI">
		<rdfs:subClassOf rdf:resource="&j2se-1_2;JavaxSwingEventAPI"/>
		<rdfs:comment xml:lang="en">JavaLibrary implementing the javax.swing.event package for J2SE 1.3</rdfs:comment>
		<rdfs:comment xml:lang="OWLManchester">platform:comprisesInterfacePart some JavaxSwingEvent</rdfs:comment>
	</owl:Class>
	<owl:Class rdf:about="&j2se-1_3;JavaxSwingPlafAPI">
		<rdfs:subClassOf rdf:resource="&j2se-1_2;JavaxSwingPlafAPI"/>
		<rdfs:comment xml:lang="en">JavaLibrary implementing the javax.swing.plaf package for J2SE 1.3</rdfs:comment>
		<rdfs:comment xml:lang="OWLManchester">platform:comprisesInterfacePart some JavaxSwingPlaf</rdfs:comment>
	</owl:Class>
	<owl:Class rdf:about="&j2se-1_3;JavaxSwingPlafBasicAPI">
		<rdfs:subClassOf rdf:resource="&j2se-1_2;JavaxSwingPlafBasicAPI"/>
		<rdfs:comment xml:lang="en">JavaLibrary implementing the javax.swing.plaf.basic package for J2SE 1.3</rdfs:comment>
		<rdfs:comment xml:lang="OWLManchester">platform:comprisesInterfacePart some JavaxSwingPlafBasic</rdfs:comment>
	</owl:Class>
	<owl:Class rdf:about="&j2se-1_3;JavaxSwingPlafMetalAPI">
		<rdfs:subClassOf rdf:resource="&j2se-1_2;JavaxSwingPlafMetalAPI"/>
		<rdfs:comment xml:lang="en">JavaLibrary implementing the javax.swing.plaf.metal package for J2SE 1.3</rdfs:comment>
		<rdfs:comment xml:lang="OWLManchester">platform:comprisesInterfacePart some JavaxSwingPlafMetal</rdfs:comment>
	</owl:Class>
	<owl:Class rdf:about="&j2se-1_3;JavaxSwingPlafMultiAPI">
		<rdfs:subClassOf rdf:resource="&j2se-1_2;JavaxSwingPlafMultiAPI"/>
		<rdfs:comment xml:lang="en">JavaLibrary implementing the javax.swing.plaf.multi package for J2SE 1.3</rdfs:comment>
		<rdfs:comment xml:lang="OWLManchester">platform:comprisesInterfacePart some JavaxSwingPlafMulti</rdfs:comment>
	</owl:Class>
	<owl:Class rdf:about="&j2se-1_3;JavaxSwingUndoAPI">
		<owl:equivalentClass rdf:resource="&j2se-1_2;JavaxSwingUndoAPI"/>
		<rdfs:subClassOf rdf:resource="&java;JavaAPI"/>
		<rdfs:comment xml:lang="en">JavaLibrary implementing the javax.swing.undo package for J2SE 1.3</rdfs:comment>
		<rdfs:comment xml:lang="OWLManchester">platform:comprisesInterfacePart some JavaxSwingUndo</rdfs:comment>
	</owl:Class>
	<owl:Class rdf:about="&j2se-1_3;JavaxSwingTreeAPI">
		<rdfs:subClassOf rdf:resource="&j2se-1_2;JavaxSwingTreeAPI"/>
		<rdfs:comment xml:lang="en">JavaLibrary implementing the javax.swing.tree package for J2SE 1.3</rdfs:comment>
		<rdfs:comment xml:lang="OWLManchester">platform:comprisesInterfacePart some JavaxSwingTree</rdfs:comment>
	</owl:Class>
	<owl:Class rdf:about="&j2se-1_3;JavaxSwingTableAPI">
		<rdfs:subClassOf rdf:resource="&j2se-1_2;JavaxSwingTableAPI"/>
		<rdfs:comment xml:lang="en">JavaLibrary implementing the javax.swing.table package for J2SE 1.3</rdfs:comment>
		<rdfs:comment xml:lang="OWLManchester">platform:comprisesInterfacePart some JavaxSwingTable</rdfs:comment>
	</owl:Class>
	<owl:Class rdf:about="&j2se-1_3;JavaxSwingBorderAPI">
		<rdfs:subClassOf rdf:resource="&j2se-1_2;JavaxSwingBorderAPI"/>
		<rdfs:comment xml:lang="en">JavaLibrary implementing the javax.swing.border package for J2SE 1.3</rdfs:comment>
		<rdfs:comment xml:lang="OWLManchester">platform:comprisesInterfacePart some JavaxSwingBorder</rdfs:comment>
	</owl:Class>
	<owl:Class rdf:about="&j2se-1_3;JavaxSwingColorchooserAPI">
		<rdfs:subClassOf rdf:resource="&j2se-1_2;JavaxSwingColorchooserAPI"/>
		<rdfs:comment xml:lang="en">JavaLibrary implementing the javax.swing.colorchooser package for J2SE 1.3</rdfs:comment>
		<rdfs:comment xml:lang="OWLManchester">platform:comprisesInterfacePart some JavaxSwingColorchooser</rdfs:comment>
	</owl:Class>
	<owl:Class rdf:about="&j2se-1_3;JavaxSwingFilechooserAPI">
		<rdfs:subClassOf rdf:resource="&j2se-1_2;JavaxSwingFilechooserAPI"/>
		<rdfs:comment xml:lang="en">JavaLibrary implementing the javax.swing.filechooser package for J2SE 1.3</rdfs:comment>
		<rdfs:comment xml:lang="OWLManchester">platform:comprisesInterfacePart some JavaxSwingFilechooser</rdfs:comment>
	</owl:Class>
	<owl:Class rdf:about="&j2se-1_3;JavaxNamingAPI">
		<rdfs:subClassOf rdf:resource="&java;JavaAPI"/>
		<rdfs:comment xml:lang="en">JavaLibrary implementing the javax.naming package for J2SE 1.3</rdfs:comment>
		<rdfs:comment xml:lang="OWLManchester">platform:comprisesInterfacePart some JavaxNaming</rdfs:comment>
	</owl:Class>
	<owl:Class rdf:about="&j2se-1_3;JavaxNamingDirectoryAPI">
		<rdfs:subClassOf rdf:resource="&java;JavaAPI"/>
		<rdfs:comment xml:lang="en">JavaLibrary implementing the javax.naming.directory package for J2SE 1.3</rdfs:comment>
		<rdfs:comment xml:lang="OWLManchester">platform:comprisesInterfacePart some JavaxNamingDirectory</rdfs:comment>
	</owl:Class>
	<owl:Class rdf:about="&j2se-1_3;JavaxNamingEventAPI">
		<rdfs:subClassOf rdf:resource="&java;JavaAPI"/>
		<rdfs:comment xml:lang="en">JavaLibrary implementing the javax.naming.event package for J2SE 1.3</rdfs:comment>
		<rdfs:comment xml:lang="OWLManchester">platform:comprisesInterfacePart some JavaxNamingEvent</rdfs:comment>
	</owl:Class>
	<owl:Class rdf:about="&j2se-1_3;JavaxNamingLdapAPI">
		<rdfs:subClassOf rdf:resource="&java;JavaAPI"/>
		<rdfs:comment xml:lang="en">JavaLibrary implementing the javax.naming.ldap package for J2SE 1.3</rdfs:comment>
		<rdfs:comment xml:lang="OWLManchester">platform:comprisesInterfacePart some JavaxNamingLdap</rdfs:comment>
	</owl:Class>
	<owl:Class rdf:about="&j2se-1_3;JavaxNamingSpiAPI">
		<rdfs:subClassOf rdf:resource="&java;JavaAPI"/>
		<rdfs:comment xml:lang="en">JavaLibrary implementing the javax.naming.spi package for J2SE 1.3</rdfs:comment>
		<rdfs:comment xml:lang="OWLManchester">platform:comprisesInterfacePart some JavaxNamingSpi</rdfs:comment>
	</owl:Class>
	<owl:Class rdf:about="&j2se-1_3;JavaxSoundMidiAPI">
		<rdfs:subClassOf rdf:resource="&java;JavaAPI"/>
		<rdfs:comment xml:lang="en">JavaLibrary implementing the javax.sound.midi package for J2SE 1.3</rdfs:comment>
		<rdfs:comment xml:lang="OWLManchester">platform:comprisesInterfacePart some JavaxSoundMidi</rdfs:comment>
	</owl:Class>
	<owl:Class rdf:about="&j2se-1_3;JavaxSoundMidiSpiAPI">
		<rdfs:subClassOf rdf:resource="&java;JavaAPI"/>
		<rdfs:comment xml:lang="en">JavaLibrary implementing the javax.sound.midi.spi package for J2SE 1.3</rdfs:comment>
		<rdfs:comment xml:lang="OWLManchester">platform:comprisesInterfacePart some JavaxSoundMidiSpi</rdfs:comment>
	</owl:Class>
	<owl:Class rdf:about="&j2se-1_3;JavaxSoundSampledAPI">
		<rdfs:subClassOf rdf:resource="&java;JavaAPI"/>
		<rdfs:comment xml:lang="en">JavaLibrary implementing the javax.sound.sampled package for J2SE 1.3</rdfs:comment>
		<rdfs:comment xml:lang="OWLManchester">platform:comprisesInterfacePart some JavaxSoundSampled</rdfs:comment>
	</owl:Class>
	<owl:Class rdf:about="&j2se-1_3;JavaxSoundSampledSpiAPI">
		<rdfs:subClassOf rdf:resource="&java;JavaAPI"/>
		<rdfs:comment xml:lang="en">JavaLibrary implementing the javax.sound.sampled.spi package for J2SE 1.3</rdfs:comment>
		<rdfs:comment xml:lang="OWLManchester">platform:comprisesInterfacePart some JavaxSoundSampledSpi</rdfs:comment>
	</owl:Class>
	<owl:Class rdf:about="&j2se-1_3;JavaxRmiAPI">
		<rdfs:subClassOf rdf:resource="&java;JavaAPI"/>
		<rdfs:comment xml:lang="en">JavaLibrary implementing the javax.rmi package for J2SE 1.3</rdfs:comment>
		<rdfs:comment xml:lang="OWLManchester">platform:comprisesInterfacePart some JavaxRmi</rdfs:comment>
	</owl:Class>
	<owl:Class rdf:about="&j2se-1_3;JavaxRmiCORBAAPI">
		<rdfs:subClassOf rdf:resource="&java;JavaAPI"/>
		<rdfs:comment xml:lang="en">JavaLibrary implementing the javax.rmi.CORBA package for J2SE 1.3</rdfs:comment>
		<rdfs:comment xml:lang="OWLManchester">platform:comprisesInterfacePart some JavaxRmiCORBA</rdfs:comment>
	</owl:Class>
	<owl:Class rdf:about="&j2se-1_3;JavaxTransactionAPI">
		<rdfs:subClassOf rdf:resource="&java;JavaAPI"/>
		<rdfs:comment xml:lang="en">JavaLibrary implementing the javax.transaction package for J2SE 1.3</rdfs:comment>
		<rdfs:comment xml:lang="OWLManchester">platform:comprisesInterfacePart some JavaxTransaction</rdfs:comment>
	</owl:Class>
	<owl:Class rdf:about="&j2se-1_3;OrgOmgCORBA_2_3API">
		<rdfs:subClassOf rdf:resource="&java;JavaAPI"/>
		<rdfs:comment xml:lang="en">JavaLibrary implementing the org.omg.CORBA_2_3 package for J2SE 1.3</rdfs:comment>
		<rdfs:comment xml:lang="OWLManchester">platform:comprisesInterfacePart some OrgOmgCORBA_2_3</rdfs:comment>
	</owl:Class>
	<owl:Class rdf:about="&j2se-1_3;OrgOmgCORBA_2_3PortableAPI">
		<rdfs:subClassOf rdf:resource="&java;JavaAPI"/>
		<rdfs:comment xml:lang="en">JavaLibrary implementing the org.omg.CORBA_2_3.portable package for J2SE 1.3</rdfs:comment>
		<rdfs:comment xml:lang="OWLManchester">platform:comprisesInterfacePart some OrgOmgCORBA_2_3Portable</rdfs:comment>
	</owl:Class>
	<owl:Class rdf:about="&j2se-1_3;OrgOmgCORBAAPI">
		<rdfs:subClassOf rdf:resource="&j2se-1_2;OrgOmgCORBAAPI"/>
		<rdfs:comment xml:lang="en">JavaLibrary implementing the org.omg.CORBA package for J2SE 1.3</rdfs:comment>
		<rdfs:comment xml:lang="OWLManchester">platform:comprisesInterfacePart some OrgOmgCORBA</rdfs:comment>
	</owl:Class>
	<owl:Class rdf:about="&j2se-1_3;OrgOmgCORBAPortableAPI">
		<rdfs:subClassOf rdf:resource="&j2se-1_2;OrgOmgCORBAPortableAPI"/>
		<rdfs:comment xml:lang="en">JavaLibrary implementing the org.omg.CORBA.portable package for J2SE 1.3</rdfs:comment>
		<rdfs:comment xml:lang="OWLManchester">platform:comprisesInterfacePart some OrgOmgCORBAPortable</rdfs:comment>
	</owl:Class>
	<owl:Class rdf:about="&j2se-1_3;OrgOmgCORBATypeCodePackageAPI">
		<owl:equivalentClass rdf:resource="&j2se-1_2;OrgOmgCORBATypeCodePackageAPI"/>
		<rdfs:subClassOf rdf:resource="&java;JavaAPI"/>
		<rdfs:comment xml:lang="en">JavaLibrary implementing the org.omg.CORBA.TypeCodePackage package for J2SE 1.3</rdfs:comment>
		<rdfs:comment xml:lang="OWLManchester">platform:comprisesInterfacePart some OrgOmgCORBATypeCodePackage</rdfs:comment>
	</owl:Class>
	<owl:Class rdf:about="&j2se-1_3;OrgOmgCORBAORBPackageAPI">
		<owl:equivalentClass rdf:resource="&j2se-1_2;OrgOmgCORBAORBPackageAPI"/>
		<rdfs:subClassOf rdf:resource="&java;JavaAPI"/>
		<rdfs:comment xml:lang="en">JavaLibrary implementing the org.omg.CORBA.ORBPackage package for J2SE 1.3</rdfs:comment>
		<rdfs:comment xml:lang="OWLManchester">platform:comprisesInterfacePart some OrgOmgCORBAORBPackage</rdfs:comment>
	</owl:Class>
	<owl:Class rdf:about="&j2se-1_3;OrgOmgCORBADynAnyPackageAPI">
		<owl:equivalentClass rdf:resource="&j2se-1_2;OrgOmgCORBADynAnyPackageAPI"/>
		<rdfs:subClassOf rdf:resource="&java;JavaAPI"/>
		<rdfs:comment xml:lang="en">JavaLibrary implementing the org.omg.CORBA.DynAnyPackage package for J2SE 1.3</rdfs:comment>
		<rdfs:comment xml:lang="OWLManchester">platform:comprisesInterfacePart some OrgOmgCORBADynAnyPackage</rdfs:comment>
	</owl:Class>
	<owl:Class rdf:about="&j2se-1_3;OrgOmgSendingContextAPI">
		<rdfs:subClassOf rdf:resource="&java;JavaAPI"/>
		<rdfs:comment xml:lang="en">JavaLibrary implementing the org.omg.SendingContext package for J2SE 1.3</rdfs:comment>
		<rdfs:comment xml:lang="OWLManchester">platform:comprisesInterfacePart some OrgOmgSendingContext</rdfs:comment>
	</owl:Class>
	<owl:Class rdf:about="&j2se-1_3;OrgOmgCosNamingAPI">
		<rdfs:subClassOf rdf:resource="&j2se-1_2;OrgOmgCosNamingAPI"/>
		<rdfs:comment xml:lang="en">JavaLibrary implementing the org.omg.CosNaming package for J2SE 1.3</rdfs:comment>
		<rdfs:comment xml:lang="OWLManchester">platform:comprisesInterfacePart some OrgOmgCosNaming</rdfs:comment>
	</owl:Class>
	<owl:Class rdf:about="&j2se-1_3;OrgOmgCosNamingNamingContextPackageAPI">
		<owl:equivalentClass rdf:resource="&j2se-1_2;OrgOmgCosNamingNamingContextPackageAPI"/>
		<rdfs:subClassOf rdf:resource="&java;JavaAPI"/>
		<rdfs:comment xml:lang="en">JavaLibrary implementing the org.omg.CosNaming.NamingContextPackage package for J2SE 1.3</rdfs:comment>
		<rdfs:comment xml:lang="OWLManchester">platform:comprisesInterfacePart some OrgOmgCosNamingNamingContextPackage</rdfs:comment>
	</owl:Class>
	<owl:Class rdf:about="&j2se-1_3;OrgOmgStubJavaRmiAPI">
		<rdfs:subClassOf rdf:resource="&java;JavaAPI"/>
		<rdfs:comment xml:lang="en">JavaLibrary implementing the org.omg.stub.java.rmi package for J2SE 1.3</rdfs:comment>
		<rdfs:comment xml:lang="OWLManchester">platform:comprisesInterfacePart some OrgOmgStubJavaRmi</rdfs:comment>
	</owl:Class>
	<j2se-1_3:JavaIo rdf:about="&j2se-1_3;theJavaIoPart">
	</j2se-1_3:JavaIo>
	<j2se-1_3:JavaLang rdf:about="&j2se-1_3;theJavaLangPart">
	</j2se-1_3:JavaLang>
	<j2se-1_3:JavaLangReflect rdf:about="&j2se-1_3;theJavaLangReflectPart">
	</j2se-1_3:JavaLangReflect>
	<j2se-1_3:JavaLangRef rdf:about="&j2se-1_3;theJavaLangRefPart">
	</j2se-1_3:JavaLangRef>
	<j2se-1_3:JavaNet rdf:about="&j2se-1_3;theJavaNetPart">
	</j2se-1_3:JavaNet>
	<j2se-1_3:JavaSecurity rdf:about="&j2se-1_3;theJavaSecurityPart">
	</j2se-1_3:JavaSecurity>
	<j2se-1_3:JavaSecurityCert rdf:about="&j2se-1_3;theJavaSecurityCertPart">
	</j2se-1_3:JavaSecurityCert>
	<j2se-1_3:JavaSecuritySpec rdf:about="&j2se-1_3;theJavaSecuritySpecPart">
	</j2se-1_3:JavaSecuritySpec>
	<j2se-1_3:JavaSecurityInterfaces rdf:about="&j2se-1_3;theJavaSecurityInterfacesPart">
	</j2se-1_3:JavaSecurityInterfaces>
	<j2se-1_3:JavaSecurityAcl rdf:about="&j2se-1_3;theJavaSecurityAclPart">
	</j2se-1_3:JavaSecurityAcl>
	<j2se-1_3:JavaUtil rdf:about="&j2se-1_3;theJavaUtilPart">
	</j2se-1_3:JavaUtil>
	<j2se-1_3:JavaUtilJar rdf:about="&j2se-1_3;theJavaUtilJarPart">
	</j2se-1_3:JavaUtilJar>
	<j2se-1_3:JavaUtilZip rdf:about="&j2se-1_3;theJavaUtilZipPart">
	</j2se-1_3:JavaUtilZip>
	<j2se-1_3:JavaMath rdf:about="&j2se-1_3;theJavaMathPart">
	</j2se-1_3:JavaMath>
	<j2se-1_3:JavaText rdf:about="&j2se-1_3;theJavaTextPart">
	</j2se-1_3:JavaText>
	<j2se-1_3:JavaTextResources rdf:about="&j2se-1_3;theJavaTextResourcesPart">
	</j2se-1_3:JavaTextResources>
	<j2se-1_3:JavaAwt rdf:about="&j2se-1_3;theJavaAwtPart">
	</j2se-1_3:JavaAwt>
	<j2se-1_3:JavaAwtGeom rdf:about="&j2se-1_3;theJavaAwtGeomPart">
	</j2se-1_3:JavaAwtGeom>
	<j2se-1_3:JavaAwtEvent rdf:about="&j2se-1_3;theJavaAwtEventPart">
	</j2se-1_3:JavaAwtEvent>
	<j2se-1_3:JavaAwtFont rdf:about="&j2se-1_3;theJavaAwtFontPart">
	</j2se-1_3:JavaAwtFont>
	<j2se-1_3:JavaAwtImage rdf:about="&j2se-1_3;theJavaAwtImagePart">
	</j2se-1_3:JavaAwtImage>
	<j2se-1_3:JavaAwtImageRenderable rdf:about="&j2se-1_3;theJavaAwtImageRenderablePart">
	</j2se-1_3:JavaAwtImageRenderable>
	<j2se-1_3:JavaAwtDnd rdf:about="&j2se-1_3;theJavaAwtDndPart">
	</j2se-1_3:JavaAwtDnd>
	<j2se-1_3:JavaAwtIm rdf:about="&j2se-1_3;theJavaAwtImPart">
	</j2se-1_3:JavaAwtIm>
	<j2se-1_3:JavaAwtImSpi rdf:about="&j2se-1_3;theJavaAwtImSpiPart">
	</j2se-1_3:JavaAwtImSpi>
	<j2se-1_3:JavaAwtColor rdf:about="&j2se-1_3;theJavaAwtColorPart">
	</j2se-1_3:JavaAwtColor>
	<j2se-1_3:JavaAwtDatatransfer rdf:about="&j2se-1_3;theJavaAwtDatatransferPart">
	</j2se-1_3:JavaAwtDatatransfer>
	<j2se-1_3:JavaAwtPrint rdf:about="&j2se-1_3;theJavaAwtPrintPart">
	</j2se-1_3:JavaAwtPrint>
	<j2se-1_3:JavaBeans rdf:about="&j2se-1_3;theJavaBeansPart">
	</j2se-1_3:JavaBeans>
	<j2se-1_3:JavaBeansBeancontext rdf:about="&j2se-1_3;theJavaBeansBeancontextPart">
	</j2se-1_3:JavaBeansBeancontext>
	<j2se-1_3:JavaApplet rdf:about="&j2se-1_3;theJavaAppletPart">
	</j2se-1_3:JavaApplet>
	<j2se-1_3:JavaRmi rdf:about="&j2se-1_3;theJavaRmiPart">
	</j2se-1_3:JavaRmi>
	<j2se-1_3:JavaRmiServer rdf:about="&j2se-1_3;theJavaRmiServerPart">
	</j2se-1_3:JavaRmiServer>
	<j2se-1_3:JavaRmiDgc rdf:about="&j2se-1_3;theJavaRmiDgcPart">
	</j2se-1_3:JavaRmiDgc>
	<j2se-1_3:JavaRmiRegistry rdf:about="&j2se-1_3;theJavaRmiRegistryPart">
	</j2se-1_3:JavaRmiRegistry>
	<j2se-1_3:JavaRmiActivation rdf:about="&j2se-1_3;theJavaRmiActivationPart">
	</j2se-1_3:JavaRmiActivation>
	<j2se-1_3:JavaSql rdf:about="&j2se-1_3;theJavaSqlPart">
	</j2se-1_3:JavaSql>
	<j2se-1_3:JavaxAccessibility rdf:about="&j2se-1_3;theJavaxAccessibilityPart">
	</j2se-1_3:JavaxAccessibility>
	<j2se-1_3:JavaxSwing rdf:about="&j2se-1_3;theJavaxSwingPart">
	</j2se-1_3:JavaxSwing>
	<j2se-1_3:JavaxSwingText rdf:about="&j2se-1_3;theJavaxSwingTextPart">
	</j2se-1_3:JavaxSwingText>
	<j2se-1_3:JavaxSwingTextHtml rdf:about="&j2se-1_3;theJavaxSwingTextHtmlPart">
	</j2se-1_3:JavaxSwingTextHtml>
	<j2se-1_3:JavaxSwingTextHtmlParser rdf:about="&j2se-1_3;theJavaxSwingTextHtmlParserPart">
	</j2se-1_3:JavaxSwingTextHtmlParser>
	<j2se-1_3:JavaxSwingTextRtf rdf:about="&j2se-1_3;theJavaxSwingTextRtfPart">
	</j2se-1_3:JavaxSwingTextRtf>
	<j2se-1_3:JavaxSwingEvent rdf:about="&j2se-1_3;theJavaxSwingEventPart">
	</j2se-1_3:JavaxSwingEvent>
	<j2se-1_3:JavaxSwingPlaf rdf:about="&j2se-1_3;theJavaxSwingPlafPart">
	</j2se-1_3:JavaxSwingPlaf>
	<j2se-1_3:JavaxSwingPlafBasic rdf:about="&j2se-1_3;theJavaxSwingPlafBasicPart">
	</j2se-1_3:JavaxSwingPlafBasic>
	<j2se-1_3:JavaxSwingPlafMetal rdf:about="&j2se-1_3;theJavaxSwingPlafMetalPart">
	</j2se-1_3:JavaxSwingPlafMetal>
	<j2se-1_3:JavaxSwingPlafMulti rdf:about="&j2se-1_3;theJavaxSwingPlafMultiPart">
	</j2se-1_3:JavaxSwingPlafMulti>
	<j2se-1_3:JavaxSwingUndo rdf:about="&j2se-1_3;theJavaxSwingUndoPart">
	</j2se-1_3:JavaxSwingUndo>
	<j2se-1_3:JavaxSwingTree rdf:about="&j2se-1_3;theJavaxSwingTreePart">
	</j2se-1_3:JavaxSwingTree>
	<j2se-1_3:JavaxSwingTable rdf:about="&j2se-1_3;theJavaxSwingTablePart">
	</j2se-1_3:JavaxSwingTable>
	<j2se-1_3:JavaxSwingBorder rdf:about="&j2se-1_3;theJavaxSwingBorderPart">
	</j2se-1_3:JavaxSwingBorder>
	<j2se-1_3:JavaxSwingColorchooser rdf:about="&j2se-1_3;theJavaxSwingColorchooserPart">
	</j2se-1_3:JavaxSwingColorchooser>
	<j2se-1_3:JavaxSwingFilechooser rdf:about="&j2se-1_3;theJavaxSwingFilechooserPart">
	</j2se-1_3:JavaxSwingFilechooser>
	<j2se-1_3:JavaxNaming rdf:about="&j2se-1_3;theJavaxNamingPart">
	</j2se-1_3:JavaxNaming>
	<j2se-1_3:JavaxNamingDirectory rdf:about="&j2se-1_3;theJavaxNamingDirectoryPart">
	</j2se-1_3:JavaxNamingDirectory>
	<j2se-1_3:JavaxNamingEvent rdf:about="&j2se-1_3;theJavaxNamingEventPart">
	</j2se-1_3:JavaxNamingEvent>
	<j2se-1_3:JavaxNamingLdap rdf:about="&j2se-1_3;theJavaxNamingLdapPart">
	</j2se-1_3:JavaxNamingLdap>
	<j2se-1_3:JavaxNamingSpi rdf:about="&j2se-1_3;theJavaxNamingSpiPart">
	</j2se-1_3:JavaxNamingSpi>
	<j2se-1_3:JavaxSoundMidi rdf:about="&j2se-1_3;theJavaxSoundMidiPart">
	</j2se-1_3:JavaxSoundMidi>
	<j2se-1_3:JavaxSoundMidiSpi rdf:about="&j2se-1_3;theJavaxSoundMidiSpiPart">
	</j2se-1_3:JavaxSoundMidiSpi>
	<j2se-1_3:JavaxSoundSampled rdf:about="&j2se-1_3;theJavaxSoundSampledPart">
	</j2se-1_3:JavaxSoundSampled>
	<j2se-1_3:JavaxSoundSampledSpi rdf:about="&j2se-1_3;theJavaxSoundSampledSpiPart">
	</j2se-1_3:JavaxSoundSampledSpi>
	<j2se-1_3:JavaxRmi rdf:about="&j2se-1_3;theJavaxRmiPart">
	</j2se-1_3:JavaxRmi>
	<j2se-1_3:JavaxRmiCORBA rdf:about="&j2se-1_3;theJavaxRmiCORBAPart">
	</j2se-1_3:JavaxRmiCORBA>
	<j2se-1_3:JavaxTransaction rdf:about="&j2se-1_3;theJavaxTransactionPart">
	</j2se-1_3:JavaxTransaction>
	<j2se-1_3:OrgOmgCORBA_2_3 rdf:about="&j2se-1_3;theOrgOmgCORBA_2_3Part">
	</j2se-1_3:OrgOmgCORBA_2_3>
	<j2se-1_3:OrgOmgCORBA_2_3Portable rdf:about="&j2se-1_3;theOrgOmgCORBA_2_3PortablePart">
	</j2se-1_3:OrgOmgCORBA_2_3Portable>
	<j2se-1_3:OrgOmgCORBA rdf:about="&j2se-1_3;theOrgOmgCORBAPart">
	</j2se-1_3:OrgOmgCORBA>
	<j2se-1_3:OrgOmgCORBAPortable rdf:about="&j2se-1_3;theOrgOmgCORBAPortablePart">
	</j2se-1_3:OrgOmgCORBAPortable>
	<j2se-1_3:OrgOmgCORBATypeCodePackage rdf:about="&j2se-1_3;theOrgOmgCORBATypeCodePackagePart">
	</j2se-1_3:OrgOmgCORBATypeCodePackage>
	<j2se-1_3:OrgOmgCORBAORBPackage rdf:about="&j2se-1_3;theOrgOmgCORBAORBPackagePart">
	</j2se-1_3:OrgOmgCORBAORBPackage>
	<j2se-1_3:OrgOmgCORBADynAnyPackage rdf:about="&j2se-1_3;theOrgOmgCORBADynAnyPackagePart">
	</j2se-1_3:OrgOmgCORBADynAnyPackage>
	<j2se-1_3:OrgOmgSendingContext rdf:about="&j2se-1_3;theOrgOmgSendingContextPart">
	</j2se-1_3:OrgOmgSendingContext>
	<j2se-1_3:OrgOmgCosNaming rdf:about="&j2se-1_3;theOrgOmgCosNamingPart">
	</j2se-1_3:OrgOmgCosNaming>
	<j2se-1_3:OrgOmgCosNamingNamingContextPackage rdf:about="&j2se-1_3;theOrgOmgCosNamingNamingContextPackagePart">
	</j2se-1_3:OrgOmgCosNamingNamingContextPackage>
	<j2se-1_3:OrgOmgStubJavaRmi rdf:about="&j2se-1_3;theOrgOmgStubJavaRmiPart">
	</j2se-1_3:OrgOmgStubJavaRmi>
	<owl:Class rdf:about="&j2se-1_3;JavaIoClassLibrary">
		<rdfs:subClassOf rdf:resource="&j2me-pp-1_0;JavaIoClassLibrary"/>
		<rdfs:subClassOf rdf:resource="&j2se-1_2;JavaIoClassLibrary"/>
		<rdfs:comment xml:lang="en">JavaLibrary implementing the java.io package for J2SE 1.3</rdfs:comment>
		<rdfs:comment xml:lang="OWLManchester">platform:implementsInterface some JavaIoAPI</rdfs:comment>
	</owl:Class>
	<owl:Class rdf:about="&j2se-1_3;JavaLangClassLibrary">
		<rdfs:subClassOf rdf:resource="&j2me-pp-1_0;JavaLangClassLibrary"/>
		<rdfs:subClassOf rdf:resource="&j2se-1_2;JavaLangClassLibrary"/>
		<rdfs:comment xml:lang="en">JavaLibrary implementing the java.lang package for J2SE 1.3</rdfs:comment>
		<rdfs:comment xml:lang="OWLManchester">platform:implementsInterface some JavaLangAPI</rdfs:comment>
	</owl:Class>
	<owl:Class rdf:about="&j2se-1_3;JavaLangReflectClassLibrary">
		<owl:equivalentClass rdf:resource="&j2me-pp-1_0;JavaLangReflectClassLibrary"/>
		<rdfs:subClassOf rdf:resource="&j2se-1_2;JavaLangReflectClassLibrary"/>
		<rdfs:comment xml:lang="en">JavaLibrary implementing the java.lang.reflect package for J2SE 1.3</rdfs:comment>
		<rdfs:comment xml:lang="OWLManchester">platform:implementsInterface some JavaLangReflectAPI</rdfs:comment>
	</owl:Class>
	<owl:Class rdf:about="&j2se-1_3;JavaLangRefClassLibrary">
		<owl:equivalentClass rdf:resource="&j2me-pp-1_0;JavaLangRefClassLibrary"/>
		<owl:equivalentClass rdf:resource="&j2se-1_2;JavaLangRefClassLibrary"/>
		<rdfs:subClassOf rdf:resource="&java;JavaClassLibrary"/>
		<rdfs:comment xml:lang="en">JavaLibrary implementing the java.lang.ref package for J2SE 1.3</rdfs:comment>
		<rdfs:comment xml:lang="OWLManchester">platform:implementsInterface some JavaLangRefAPI</rdfs:comment>
	</owl:Class>
	<owl:Class rdf:about="&j2se-1_3;JavaNetClassLibrary">
		<rdfs:subClassOf rdf:resource="&j2me-pp-1_0;JavaNetClassLibrary"/>
		<rdfs:subClassOf rdf:resource="&j2se-1_2;JavaNetClassLibrary"/>
		<rdfs:comment xml:lang="en">JavaLibrary implementing the java.net package for J2SE 1.3</rdfs:comment>
		<rdfs:comment xml:lang="OWLManchester">platform:implementsInterface some JavaNetAPI</rdfs:comment>
	</owl:Class>
	<owl:Class rdf:about="&j2se-1_3;JavaSecurityClassLibrary">
		<rdfs:subClassOf rdf:resource="&j2me-pp-1_0;JavaSecurityClassLibrary"/>
		<rdfs:subClassOf rdf:resource="&j2se-1_2;JavaSecurityClassLibrary"/>
		<rdfs:comment xml:lang="en">JavaLibrary implementing the java.security package for J2SE 1.3</rdfs:comment>
		<rdfs:comment xml:lang="OWLManchester">platform:implementsInterface some JavaSecurityAPI</rdfs:comment>
	</owl:Class>
	<owl:Class rdf:about="&j2se-1_3;JavaSecurityCertClassLibrary">
		<owl:equivalentClass rdf:resource="&j2me-pp-1_0;JavaSecurityCertClassLibrary"/>
		<rdfs:subClassOf rdf:resource="&j2se-1_2;JavaSecurityCertClassLibrary"/>
		<rdfs:comment xml:lang="en">JavaLibrary implementing the java.security.cert package for J2SE 1.3</rdfs:comment>
		<rdfs:comment xml:lang="OWLManchester">platform:implementsInterface some JavaSecurityCertAPI</rdfs:comment>
	</owl:Class>
	<owl:Class rdf:about="&j2se-1_3;JavaSecuritySpecClassLibrary">
		<owl:equivalentClass rdf:resource="&j2me-pp-1_0;JavaSecuritySpecClassLibrary"/>
		<rdfs:subClassOf rdf:resource="&j2se-1_2;JavaSecuritySpecClassLibrary"/>
		<rdfs:comment xml:lang="en">JavaLibrary implementing the java.security.spec package for J2SE 1.3</rdfs:comment>
		<rdfs:comment xml:lang="OWLManchester">platform:implementsInterface some JavaSecuritySpecAPI</rdfs:comment>
	</owl:Class>
	<owl:Class rdf:about="&j2se-1_3;JavaSecurityInterfacesClassLibrary">
		<owl:equivalentClass rdf:resource="&j2me-pp-1_0;JavaSecurityInterfacesClassLibrary"/>
		<rdfs:subClassOf rdf:resource="&j2se-1_2;JavaSecurityInterfacesClassLibrary"/>
		<rdfs:comment xml:lang="en">JavaLibrary implementing the java.security.interfaces package for J2SE 1.3</rdfs:comment>
		<rdfs:comment xml:lang="OWLManchester">platform:implementsInterface some JavaSecurityInterfacesAPI</rdfs:comment>
	</owl:Class>
	<owl:Class rdf:about="&j2se-1_3;JavaSecurityAclClassLibrary">
		<owl:equivalentClass rdf:resource="&j2me-pp-1_0;JavaSecurityAclClassLibrary"/>
		<owl:equivalentClass rdf:resource="&j2se-1_2;JavaSecurityAclClassLibrary"/>
		<rdfs:subClassOf rdf:resource="&java;JavaClassLibrary"/>
		<rdfs:comment xml:lang="en">JavaLibrary implementing the java.security.acl package for J2SE 1.3</rdfs:comment>
		<rdfs:comment xml:lang="OWLManchester">platform:implementsInterface some JavaSecurityAclAPI</rdfs:comment>
	</owl:Class>
	<owl:Class rdf:about="&j2se-1_3;JavaUtilClassLibrary">
		<rdfs:subClassOf rdf:resource="&j2me-pp-1_0;JavaUtilClassLibrary"/>
		<rdfs:subClassOf rdf:resource="&j2se-1_2;JavaUtilClassLibrary"/>
		<rdfs:comment xml:lang="en">JavaLibrary implementing the java.util package for J2SE 1.3</rdfs:comment>
		<rdfs:comment xml:lang="OWLManchester">platform:implementsInterface some JavaUtilAPI</rdfs:comment>
	</owl:Class>
	<owl:Class rdf:about="&j2se-1_3;JavaUtilJarClassLibrary">
		<owl:equivalentClass rdf:resource="&j2me-pp-1_0;JavaUtilJarClassLibrary"/>
		<rdfs:subClassOf rdf:resource="&j2se-1_2;JavaUtilJarClassLibrary"/>
		<rdfs:comment xml:lang="en">JavaLibrary implementing the java.util.jar package for J2SE 1.3</rdfs:comment>
		<rdfs:comment xml:lang="OWLManchester">platform:implementsInterface some JavaUtilJarAPI</rdfs:comment>
	</owl:Class>
	<owl:Class rdf:about="&j2se-1_3;JavaUtilZipClassLibrary">
		<owl:equivalentClass rdf:resource="&j2me-pp-1_0;JavaUtilZipClassLibrary"/>
		<rdfs:subClassOf rdf:resource="&j2se-1_2;JavaUtilZipClassLibrary"/>
		<rdfs:comment xml:lang="en">JavaLibrary implementing the java.util.zip package for J2SE 1.3</rdfs:comment>
		<rdfs:comment xml:lang="OWLManchester">platform:implementsInterface some JavaUtilZipAPI</rdfs:comment>
	</owl:Class>
	<owl:Class rdf:about="&j2se-1_3;JavaMathClassLibrary">
		<owl:equivalentClass rdf:resource="&j2me-pp-1_0;JavaMathClassLibrary"/>
		<owl:equivalentClass rdf:resource="&j2se-1_2;JavaMathClassLibrary"/>
		<rdfs:subClassOf rdf:resource="&java;JavaClassLibrary"/>
		<rdfs:comment xml:lang="en">JavaLibrary implementing the java.math package for J2SE 1.3</rdfs:comment>
		<rdfs:comment xml:lang="OWLManchester">platform:implementsInterface some JavaMathAPI</rdfs:comment>
	</owl:Class>
	<owl:Class rdf:about="&j2se-1_3;JavaTextClassLibrary">
		<owl:equivalentClass rdf:resource="&j2me-pp-1_0;JavaTextClassLibrary"/>
		<rdfs:subClassOf rdf:resource="&java;JavaClassLibrary"/>
		<rdfs:comment xml:lang="en">JavaLibrary implementing the java.text package for J2SE 1.3</rdfs:comment>
		<rdfs:comment xml:lang="OWLManchester">platform:implementsInterface some JavaTextAPI</rdfs:comment>
	</owl:Class>
	<owl:Class rdf:about="&j2se-1_3;JavaTextResourcesClassLibrary">
		<owl:equivalentClass rdf:resource="&j2me-pp-1_0;JavaTextResourcesClassLibrary"/>
		<rdfs:subClassOf rdf:resource="&java;JavaClassLibrary"/>
		<rdfs:comment xml:lang="en">JavaLibrary implementing the java.text.resources package for J2SE 1.3</rdfs:comment>
		<rdfs:comment xml:lang="OWLManchester">platform:implementsInterface some JavaTextResourcesAPI</rdfs:comment>
	</owl:Class>
	<owl:Class rdf:about="&j2se-1_3;JavaAwtClassLibrary">
		<rdfs:subClassOf rdf:resource="&j2me-pp-1_0;JavaAwtClassLibrary"/>
		<rdfs:subClassOf rdf:resource="&j2se-1_2;JavaAwtClassLibrary"/>
		<rdfs:comment xml:lang="en">JavaLibrary implementing the java.awt package for J2SE 1.3</rdfs:comment>
		<rdfs:comment xml:lang="OWLManchester">platform:implementsInterface some JavaAwtAPI</rdfs:comment>
	</owl:Class>
	<owl:Class rdf:about="&j2se-1_3;JavaAwtGeomClassLibrary">
		<rdfs:subClassOf rdf:resource="&j2se-1_2;JavaAwtGeomClassLibrary"/>
		<rdfs:comment xml:lang="en">JavaLibrary implementing the java.awt.geom package for J2SE 1.3</rdfs:comment>
		<rdfs:comment xml:lang="OWLManchester">platform:implementsInterface some JavaAwtGeomAPI</rdfs:comment>
	</owl:Class>
	<owl:Class rdf:about="&j2se-1_3;JavaAwtEventClassLibrary">
		<rdfs:subClassOf rdf:resource="&j2me-pp-1_0;JavaAwtEventClassLibrary"/>
		<rdfs:subClassOf rdf:resource="&j2se-1_2;JavaAwtEventClassLibrary"/>
		<rdfs:comment xml:lang="en">JavaLibrary implementing the java.awt.event package for J2SE 1.3</rdfs:comment>
		<rdfs:comment xml:lang="OWLManchester">platform:implementsInterface some JavaAwtEventAPI</rdfs:comment>
	</owl:Class>
	<owl:Class rdf:about="&j2se-1_3;JavaAwtFontClassLibrary">
		<rdfs:subClassOf rdf:resource="&java;JavaClassLibrary"/>
		<rdfs:comment xml:lang="en">JavaLibrary implementing the java.awt.font package for J2SE 1.3</rdfs:comment>
		<rdfs:comment xml:lang="OWLManchester">platform:implementsInterface some JavaAwtFontAPI</rdfs:comment>
	</owl:Class>
	<owl:Class rdf:about="&j2se-1_3;JavaAwtImageClassLibrary">
		<rdfs:subClassOf rdf:resource="&j2me-pp-1_0;JavaAwtImageClassLibrary"/>
		<rdfs:subClassOf rdf:resource="&j2se-1_2;JavaAwtImageClassLibrary"/>
		<rdfs:comment xml:lang="en">JavaLibrary implementing the java.awt.image package for J2SE 1.3</rdfs:comment>
		<rdfs:comment xml:lang="OWLManchester">platform:implementsInterface some JavaAwtImageAPI</rdfs:comment>
	</owl:Class>
	<owl:Class rdf:about="&j2se-1_3;JavaAwtImageRenderableClassLibrary">
		<rdfs:subClassOf rdf:resource="&j2se-1_2;JavaAwtImageRenderableClassLibrary"/>
		<rdfs:comment xml:lang="en">JavaLibrary implementing the java.awt.image.renderable package for J2SE 1.3</rdfs:comment>
		<rdfs:comment xml:lang="OWLManchester">platform:implementsInterface some JavaAwtImageRenderableAPI</rdfs:comment>
	</owl:Class>
	<owl:Class rdf:about="&j2se-1_3;JavaAwtDndClassLibrary">
		<owl:equivalentClass rdf:resource="&j2se-1_2;JavaAwtDndClassLibrary"/>
		<rdfs:subClassOf rdf:resource="&java;JavaClassLibrary"/>
		<rdfs:comment xml:lang="en">JavaLibrary implementing the java.awt.dnd package for J2SE 1.3</rdfs:comment>
		<rdfs:comment xml:lang="OWLManchester">platform:implementsInterface some JavaAwtDndAPI</rdfs:comment>
	</owl:Class>
	<owl:Class rdf:about="&j2se-1_3;JavaAwtImClassLibrary">
		<rdfs:subClassOf rdf:resource="&j2se-1_2;JavaAwtImClassLibrary"/>
		<rdfs:comment xml:lang="en">JavaLibrary implementing the java.awt.im package for J2SE 1.3</rdfs:comment>
		<rdfs:comment xml:lang="OWLManchester">platform:implementsInterface some JavaAwtImAPI</rdfs:comment>
	</owl:Class>
	<owl:Class rdf:about="&j2se-1_3;JavaAwtImSpiClassLibrary">
		<rdfs:subClassOf rdf:resource="&java;JavaClassLibrary"/>
		<rdfs:comment xml:lang="en">JavaLibrary implementing the java.awt.im.spi package for J2SE 1.3</rdfs:comment>
		<rdfs:comment xml:lang="OWLManchester">platform:implementsInterface some JavaAwtImSpiAPI</rdfs:comment>
	</owl:Class>
	<owl:Class rdf:about="&j2se-1_3;JavaAwtColorClassLibrary">
		<rdfs:subClassOf rdf:resource="&j2me-pp-1_0;JavaAwtColorClassLibrary"/>
		<rdfs:subClassOf rdf:resource="&j2se-1_2;JavaAwtColorClassLibrary"/>
		<rdfs:comment xml:lang="en">JavaLibrary implementing the java.awt.color package for J2SE 1.3</rdfs:comment>
		<rdfs:comment xml:lang="OWLManchester">platform:implementsInterface some JavaAwtColorAPI</rdfs:comment>
	</owl:Class>
	<owl:Class rdf:about="&j2se-1_3;JavaAwtDatatransferClassLibrary">
		<rdfs:subClassOf rdf:resource="&j2me-pp-1_0;JavaAwtDatatransferClassLibrary"/>
		<rdfs:subClassOf rdf:resource="&j2se-1_2;JavaAwtDatatransferClassLibrary"/>
		<rdfs:comment xml:lang="en">JavaLibrary implementing the java.awt.datatransfer package for J2SE 1.3</rdfs:comment>
		<rdfs:comment xml:lang="OWLManchester">platform:implementsInterface some JavaAwtDatatransferAPI</rdfs:comment>
	</owl:Class>
	<owl:Class rdf:about="&j2se-1_3;JavaAwtPrintClassLibrary">
		<owl:equivalentClass rdf:resource="&j2se-1_2;JavaAwtPrintClassLibrary"/>
		<rdfs:subClassOf rdf:resource="&java;JavaClassLibrary"/>
		<rdfs:comment xml:lang="en">JavaLibrary implementing the java.awt.print package for J2SE 1.3</rdfs:comment>
		<rdfs:comment xml:lang="OWLManchester">platform:implementsInterface some JavaAwtPrintAPI</rdfs:comment>
	</owl:Class>
	<owl:Class rdf:about="&j2se-1_3;JavaBeansClassLibrary">
		<owl:equivalentClass rdf:resource="&j2se-1_2;JavaBeansClassLibrary"/>
		<rdfs:subClassOf rdf:resource="&j2me-pp-1_0;JavaBeansClassLibrary"/>
		<rdfs:comment xml:lang="en">JavaLibrary implementing the java.beans package for J2SE 1.3</rdfs:comment>
		<rdfs:comment xml:lang="OWLManchester">platform:implementsInterface some JavaBeansAPI</rdfs:comment>
	</owl:Class>
	<owl:Class rdf:about="&j2se-1_3;JavaBeansBeancontextClassLibrary">
		<owl:equivalentClass rdf:resource="&j2se-1_2;JavaBeansBeancontextClassLibrary"/>
		<rdfs:subClassOf rdf:resource="&java;JavaClassLibrary"/>
		<rdfs:comment xml:lang="en">JavaLibrary implementing the java.beans.beancontext package for J2SE 1.3</rdfs:comment>
		<rdfs:comment xml:lang="OWLManchester">platform:implementsInterface some JavaBeansBeancontextAPI</rdfs:comment>
	</owl:Class>
	<owl:Class rdf:about="&j2se-1_3;JavaAppletClassLibrary">
		<rdfs:subClassOf rdf:resource="&j2me-pp-1_0;JavaAppletClassLibrary"/>
		<rdfs:subClassOf rdf:resource="&j2se-1_2;JavaAppletClassLibrary"/>
		<rdfs:comment xml:lang="en">JavaLibrary implementing the java.applet package for J2SE 1.3</rdfs:comment>
		<rdfs:comment xml:lang="OWLManchester">platform:implementsInterface some JavaAppletAPI</rdfs:comment>
	</owl:Class>
	<owl:Class rdf:about="&j2se-1_3;JavaRmiClassLibrary">
		<owl:equivalentClass rdf:resource="&j2se-1_2;JavaRmiClassLibrary"/>
		<rdfs:subClassOf rdf:resource="&j2me-pp-1_0;JavaRmiClassLibrary"/>
		<rdfs:comment xml:lang="en">JavaLibrary implementing the java.rmi package for J2SE 1.3</rdfs:comment>
		<rdfs:comment xml:lang="OWLManchester">platform:implementsInterface some JavaRmiAPI</rdfs:comment>
	</owl:Class>
	<owl:Class rdf:about="&j2se-1_3;JavaRmiServerClassLibrary">
		<rdfs:subClassOf rdf:resource="&j2se-1_2;JavaRmiServerClassLibrary"/>
		<rdfs:comment xml:lang="en">JavaLibrary implementing the java.rmi.server package for J2SE 1.3</rdfs:comment>
		<rdfs:comment xml:lang="OWLManchester">platform:implementsInterface some JavaRmiServerAPI</rdfs:comment>
	</owl:Class>
	<owl:Class rdf:about="&j2se-1_3;JavaRmiDgcClassLibrary">
		<owl:equivalentClass rdf:resource="&j2se-1_2;JavaRmiDgcClassLibrary"/>
		<rdfs:subClassOf rdf:resource="&java;JavaClassLibrary"/>
		<rdfs:comment xml:lang="en">JavaLibrary implementing the java.rmi.dgc package for J2SE 1.3</rdfs:comment>
		<rdfs:comment xml:lang="OWLManchester">platform:implementsInterface some JavaRmiDgcAPI</rdfs:comment>
	</owl:Class>
	<owl:Class rdf:about="&j2se-1_3;JavaRmiRegistryClassLibrary">
		<owl:equivalentClass rdf:resource="&j2se-1_2;JavaRmiRegistryClassLibrary"/>
		<rdfs:subClassOf rdf:resource="&j2me-pp-1_0;JavaRmiRegistryClassLibrary"/>
		<rdfs:comment xml:lang="en">JavaLibrary implementing the java.rmi.registry package for J2SE 1.3</rdfs:comment>
		<rdfs:comment xml:lang="OWLManchester">platform:implementsInterface some JavaRmiRegistryAPI</rdfs:comment>
	</owl:Class>
	<owl:Class rdf:about="&j2se-1_3;JavaRmiActivationClassLibrary">
		<owl:equivalentClass rdf:resource="&j2se-1_2;JavaRmiActivationClassLibrary"/>
		<rdfs:subClassOf rdf:resource="&java;JavaClassLibrary"/>
		<rdfs:comment xml:lang="en">JavaLibrary implementing the java.rmi.activation package for J2SE 1.3</rdfs:comment>
		<rdfs:comment xml:lang="OWLManchester">platform:implementsInterface some JavaRmiActivationAPI</rdfs:comment>
	</owl:Class>
	<owl:Class rdf:about="&j2se-1_3;JavaSqlClassLibrary">
		<rdfs:subClassOf rdf:resource="&j2se-1_2;JavaSqlClassLibrary"/>
		<rdfs:comment xml:lang="en">JavaLibrary implementing the java.sql package for J2SE 1.3</rdfs:comment>
		<rdfs:comment xml:lang="OWLManchester">platform:implementsInterface some JavaSqlAPI</rdfs:comment>
	</owl:Class>
	<owl:Class rdf:about="&j2se-1_3;JavaxAccessibilityClassLibrary">
		<rdfs:subClassOf rdf:resource="&j2se-1_2;JavaxAccessibilityClassLibrary"/>
		<rdfs:comment xml:lang="en">JavaLibrary implementing the javax.accessibility package for J2SE 1.3</rdfs:comment>
		<rdfs:comment xml:lang="OWLManchester">platform:implementsInterface some JavaxAccessibilityAPI</rdfs:comment>
	</owl:Class>
	<owl:Class rdf:about="&j2se-1_3;JavaxSwingClassLibrary">
		<rdfs:subClassOf rdf:resource="&java;JavaClassLibrary"/>
		<rdfs:comment xml:lang="en">JavaLibrary implementing the javax.swing package for J2SE 1.3</rdfs:comment>
		<rdfs:comment xml:lang="OWLManchester">platform:implementsInterface some JavaxSwingAPI</rdfs:comment>
	</owl:Class>
	<owl:Class rdf:about="&j2se-1_3;JavaxSwingTextClassLibrary">
		<rdfs:subClassOf rdf:resource="&j2se-1_2;JavaxSwingTextClassLibrary"/>
		<rdfs:comment xml:lang="en">JavaLibrary implementing the javax.swing.text package for J2SE 1.3</rdfs:comment>
		<rdfs:comment xml:lang="OWLManchester">platform:implementsInterface some JavaxSwingTextAPI</rdfs:comment>
	</owl:Class>
	<owl:Class rdf:about="&j2se-1_3;JavaxSwingTextHtmlClassLibrary">
		<rdfs:subClassOf rdf:resource="&j2se-1_2;JavaxSwingTextHtmlClassLibrary"/>
		<rdfs:comment xml:lang="en">JavaLibrary implementing the javax.swing.text.html package for J2SE 1.3</rdfs:comment>
		<rdfs:comment xml:lang="OWLManchester">platform:implementsInterface some JavaxSwingTextHtmlAPI</rdfs:comment>
	</owl:Class>
	<owl:Class rdf:about="&j2se-1_3;JavaxSwingTextHtmlParserClassLibrary">
		<rdfs:subClassOf rdf:resource="&j2se-1_2;JavaxSwingTextHtmlParserClassLibrary"/>
		<rdfs:comment xml:lang="en">JavaLibrary implementing the javax.swing.text.html.parser package for J2SE 1.3</rdfs:comment>
		<rdfs:comment xml:lang="OWLManchester">platform:implementsInterface some JavaxSwingTextHtmlParserAPI</rdfs:comment>
	</owl:Class>
	<owl:Class rdf:about="&j2se-1_3;JavaxSwingTextRtfClassLibrary">
		<owl:equivalentClass rdf:resource="&j2se-1_2;JavaxSwingTextRtfClassLibrary"/>
		<rdfs:subClassOf rdf:resource="&java;JavaClassLibrary"/>
		<rdfs:comment xml:lang="en">JavaLibrary implementing the javax.swing.text.rtf package for J2SE 1.3</rdfs:comment>
		<rdfs:comment xml:lang="OWLManchester">platform:implementsInterface some JavaxSwingTextRtfAPI</rdfs:comment>
	</owl:Class>
	<owl:Class rdf:about="&j2se-1_3;JavaxSwingEventClassLibrary">
		<rdfs:subClassOf rdf:resource="&j2se-1_2;JavaxSwingEventClassLibrary"/>
		<rdfs:comment xml:lang="en">JavaLibrary implementing the javax.swing.event package for J2SE 1.3</rdfs:comment>
		<rdfs:comment xml:lang="OWLManchester">platform:implementsInterface some JavaxSwingEventAPI</rdfs:comment>
	</owl:Class>
	<owl:Class rdf:about="&j2se-1_3;JavaxSwingPlafClassLibrary">
		<rdfs:subClassOf rdf:resource="&j2se-1_2;JavaxSwingPlafClassLibrary"/>
		<rdfs:comment xml:lang="en">JavaLibrary implementing the javax.swing.plaf package for J2SE 1.3</rdfs:comment>
		<rdfs:comment xml:lang="OWLManchester">platform:implementsInterface some JavaxSwingPlafAPI</rdfs:comment>
	</owl:Class>
	<owl:Class rdf:about="&j2se-1_3;JavaxSwingPlafBasicClassLibrary">
		<rdfs:subClassOf rdf:resource="&j2se-1_2;JavaxSwingPlafBasicClassLibrary"/>
		<rdfs:comment xml:lang="en">JavaLibrary implementing the javax.swing.plaf.basic package for J2SE 1.3</rdfs:comment>
		<rdfs:comment xml:lang="OWLManchester">platform:implementsInterface some JavaxSwingPlafBasicAPI</rdfs:comment>
	</owl:Class>
	<owl:Class rdf:about="&j2se-1_3;JavaxSwingPlafMetalClassLibrary">
		<rdfs:subClassOf rdf:resource="&j2se-1_2;JavaxSwingPlafMetalClassLibrary"/>
		<rdfs:comment xml:lang="en">JavaLibrary implementing the javax.swing.plaf.metal package for J2SE 1.3</rdfs:comment>
		<rdfs:comment xml:lang="OWLManchester">platform:implementsInterface some JavaxSwingPlafMetalAPI</rdfs:comment>
	</owl:Class>
	<owl:Class rdf:about="&j2se-1_3;JavaxSwingPlafMultiClassLibrary">
		<rdfs:subClassOf rdf:resource="&j2se-1_2;JavaxSwingPlafMultiClassLibrary"/>
		<rdfs:comment xml:lang="en">JavaLibrary implementing the javax.swing.plaf.multi package for J2SE 1.3</rdfs:comment>
		<rdfs:comment xml:lang="OWLManchester">platform:implementsInterface some JavaxSwingPlafMultiAPI</rdfs:comment>
	</owl:Class>
	<owl:Class rdf:about="&j2se-1_3;JavaxSwingUndoClassLibrary">
		<owl:equivalentClass rdf:resource="&j2se-1_2;JavaxSwingUndoClassLibrary"/>
		<rdfs:subClassOf rdf:resource="&java;JavaClassLibrary"/>
		<rdfs:comment xml:lang="en">JavaLibrary implementing the javax.swing.undo package for J2SE 1.3</rdfs:comment>
		<rdfs:comment xml:lang="OWLManchester">platform:implementsInterface some JavaxSwingUndoAPI</rdfs:comment>
	</owl:Class>
	<owl:Class rdf:about="&j2se-1_3;JavaxSwingTreeClassLibrary">
		<rdfs:subClassOf rdf:resource="&j2se-1_2;JavaxSwingTreeClassLibrary"/>
		<rdfs:comment xml:lang="en">JavaLibrary implementing the javax.swing.tree package for J2SE 1.3</rdfs:comment>
		<rdfs:comment xml:lang="OWLManchester">platform:implementsInterface some JavaxSwingTreeAPI</rdfs:comment>
	</owl:Class>
	<owl:Class rdf:about="&j2se-1_3;JavaxSwingTableClassLibrary">
		<rdfs:subClassOf rdf:resource="&j2se-1_2;JavaxSwingTableClassLibrary"/>
		<rdfs:comment xml:lang="en">JavaLibrary implementing the javax.swing.table package for J2SE 1.3</rdfs:comment>
		<rdfs:comment xml:lang="OWLManchester">platform:implementsInterface some JavaxSwingTableAPI</rdfs:comment>
	</owl:Class>
	<owl:Class rdf:about="&j2se-1_3;JavaxSwingBorderClassLibrary">
		<rdfs:subClassOf rdf:resource="&j2se-1_2;JavaxSwingBorderClassLibrary"/>
		<rdfs:comment xml:lang="en">JavaLibrary implementing the javax.swing.border package for J2SE 1.3</rdfs:comment>
		<rdfs:comment xml:lang="OWLManchester">platform:implementsInterface some JavaxSwingBorderAPI</rdfs:comment>
	</owl:Class>
	<owl:Class rdf:about="&j2se-1_3;JavaxSwingColorchooserClassLibrary">
		<rdfs:subClassOf rdf:resource="&j2se-1_2;JavaxSwingColorchooserClassLibrary"/>
		<rdfs:comment xml:lang="en">JavaLibrary implementing the javax.swing.colorchooser package for J2SE 1.3</rdfs:comment>
		<rdfs:comment xml:lang="OWLManchester">platform:implementsInterface some JavaxSwingColorchooserAPI</rdfs:comment>
	</owl:Class>
	<owl:Class rdf:about="&j2se-1_3;JavaxSwingFilechooserClassLibrary">
		<rdfs:subClassOf rdf:resource="&j2se-1_2;JavaxSwingFilechooserClassLibrary"/>
		<rdfs:comment xml:lang="en">JavaLibrary implementing the javax.swing.filechooser package for J2SE 1.3</rdfs:comment>
		<rdfs:comment xml:lang="OWLManchester">platform:implementsInterface some JavaxSwingFilechooserAPI</rdfs:comment>
	</owl:Class>
	<owl:Class rdf:about="&j2se-1_3;JavaxNamingClassLibrary">
		<rdfs:subClassOf rdf:resource="&java;JavaClassLibrary"/>
		<rdfs:comment xml:lang="en">JavaLibrary implementing the javax.naming package for J2SE 1.3</rdfs:comment>
		<rdfs:comment xml:lang="OWLManchester">platform:implementsInterface some JavaxNamingAPI</rdfs:comment>
	</owl:Class>
	<owl:Class rdf:about="&j2se-1_3;JavaxNamingDirectoryClassLibrary">
		<rdfs:subClassOf rdf:resource="&java;JavaClassLibrary"/>
		<rdfs:comment xml:lang="en">JavaLibrary implementing the javax.naming.directory package for J2SE 1.3</rdfs:comment>
		<rdfs:comment xml:lang="OWLManchester">platform:implementsInterface some JavaxNamingDirectoryAPI</rdfs:comment>
	</owl:Class>
	<owl:Class rdf:about="&j2se-1_3;JavaxNamingEventClassLibrary">
		<rdfs:subClassOf rdf:resource="&java;JavaClassLibrary"/>
		<rdfs:comment xml:lang="en">JavaLibrary implementing the javax.naming.event package for J2SE 1.3</rdfs:comment>
		<rdfs:comment xml:lang="OWLManchester">platform:implementsInterface some JavaxNamingEventAPI</rdfs:comment>
	</owl:Class>
	<owl:Class rdf:about="&j2se-1_3;JavaxNamingLdapClassLibrary">
		<rdfs:subClassOf rdf:resource="&java;JavaClassLibrary"/>
		<rdfs:comment xml:lang="en">JavaLibrary implementing the javax.naming.ldap package for J2SE 1.3</rdfs:comment>
		<rdfs:comment xml:lang="OWLManchester">platform:implementsInterface some JavaxNamingLdapAPI</rdfs:comment>
	</owl:Class>
	<owl:Class rdf:about="&j2se-1_3;JavaxNamingSpiClassLibrary">
		<rdfs:subClassOf rdf:resource="&java;JavaClassLibrary"/>
		<rdfs:comment xml:lang="en">JavaLibrary implementing the javax.naming.spi package for J2SE 1.3</rdfs:comment>
		<rdfs:comment xml:lang="OWLManchester">platform:implementsInterface some JavaxNamingSpiAPI</rdfs:comment>
	</owl:Class>
	<owl:Class rdf:about="&j2se-1_3;JavaxSoundMidiClassLibrary">
		<rdfs:subClassOf rdf:resource="&java;JavaClassLibrary"/>
		<rdfs:comment xml:lang="en">JavaLibrary implementing the javax.sound.midi package for J2SE 1.3</rdfs:comment>
		<rdfs:comment xml:lang="OWLManchester">platform:implementsInterface some JavaxSoundMidiAPI</rdfs:comment>
	</owl:Class>
	<owl:Class rdf:about="&j2se-1_3;JavaxSoundMidiSpiClassLibrary">
		<rdfs:subClassOf rdf:resource="&java;JavaClassLibrary"/>
		<rdfs:comment xml:lang="en">JavaLibrary implementing the javax.sound.midi.spi package for J2SE 1.3</rdfs:comment>
		<rdfs:comment xml:lang="OWLManchester">platform:implementsInterface some JavaxSoundMidiSpiAPI</rdfs:comment>
	</owl:Class>
	<owl:Class rdf:about="&j2se-1_3;JavaxSoundSampledClassLibrary">
		<rdfs:subClassOf rdf:resource="&java;JavaClassLibrary"/>
		<rdfs:comment xml:lang="en">JavaLibrary implementing the javax.sound.sampled package for J2SE 1.3</rdfs:comment>
		<rdfs:comment xml:lang="OWLManchester">platform:implementsInterface some JavaxSoundSampledAPI</rdfs:comment>
	</owl:Class>
	<owl:Class rdf:about="&j2se-1_3;JavaxSoundSampledSpiClassLibrary">
		<rdfs:subClassOf rdf:resource="&java;JavaClassLibrary"/>
		<rdfs:comment xml:lang="en">JavaLibrary implementing the javax.sound.sampled.spi package for J2SE 1.3</rdfs:comment>
		<rdfs:comment xml:lang="OWLManchester">platform:implementsInterface some JavaxSoundSampledSpiAPI</rdfs:comment>
	</owl:Class>
	<owl:Class rdf:about="&j2se-1_3;JavaxRmiClassLibrary">
		<rdfs:subClassOf rdf:resource="&java;JavaClassLibrary"/>
		<rdfs:comment xml:lang="en">JavaLibrary implementing the javax.rmi package for J2SE 1.3</rdfs:comment>
		<rdfs:comment xml:lang="OWLManchester">platform:implementsInterface some JavaxRmiAPI</rdfs:comment>
	</owl:Class>
	<owl:Class rdf:about="&j2se-1_3;JavaxRmiCORBAClassLibrary">
		<rdfs:subClassOf rdf:resource="&java;JavaClassLibrary"/>
		<rdfs:comment xml:lang="en">JavaLibrary implementing the javax.rmi.CORBA package for J2SE 1.3</rdfs:comment>
		<rdfs:comment xml:lang="OWLManchester">platform:implementsInterface some JavaxRmiCORBAAPI</rdfs:comment>
	</owl:Class>
	<owl:Class rdf:about="&j2se-1_3;JavaxTransactionClassLibrary">
		<rdfs:subClassOf rdf:resource="&java;JavaClassLibrary"/>
		<rdfs:comment xml:lang="en">JavaLibrary implementing the javax.transaction package for J2SE 1.3</rdfs:comment>
		<rdfs:comment xml:lang="OWLManchester">platform:implementsInterface some JavaxTransactionAPI</rdfs:comment>
	</owl:Class>
	<owl:Class rdf:about="&j2se-1_3;OrgOmgCORBA_2_3ClassLibrary">
		<rdfs:subClassOf rdf:resource="&java;JavaClassLibrary"/>
		<rdfs:comment xml:lang="en">JavaLibrary implementing the org.omg.CORBA_2_3 package for J2SE 1.3</rdfs:comment>
		<rdfs:comment xml:lang="OWLManchester">platform:implementsInterface some OrgOmgCORBA_2_3API</rdfs:comment>
	</owl:Class>
	<owl:Class rdf:about="&j2se-1_3;OrgOmgCORBA_2_3PortableClassLibrary">
		<rdfs:subClassOf rdf:resource="&java;JavaClassLibrary"/>
		<rdfs:comment xml:lang="en">JavaLibrary implementing the org.omg.CORBA_2_3.portable package for J2SE 1.3</rdfs:comment>
		<rdfs:comment xml:lang="OWLManchester">platform:implementsInterface some OrgOmgCORBA_2_3PortableAPI</rdfs:comment>
	</owl:Class>
	<owl:Class rdf:about="&j2se-1_3;OrgOmgCORBAClassLibrary">
		<rdfs:subClassOf rdf:resource="&j2se-1_2;OrgOmgCORBAClassLibrary"/>
		<rdfs:comment xml:lang="en">JavaLibrary implementing the org.omg.CORBA package for J2SE 1.3</rdfs:comment>
		<rdfs:comment xml:lang="OWLManchester">platform:implementsInterface some OrgOmgCORBAAPI</rdfs:comment>
	</owl:Class>
	<owl:Class rdf:about="&j2se-1_3;OrgOmgCORBAPortableClassLibrary">
		<rdfs:subClassOf rdf:resource="&j2se-1_2;OrgOmgCORBAPortableClassLibrary"/>
		<rdfs:comment xml:lang="en">JavaLibrary implementing the org.omg.CORBA.portable package for J2SE 1.3</rdfs:comment>
		<rdfs:comment xml:lang="OWLManchester">platform:implementsInterface some OrgOmgCORBAPortableAPI</rdfs:comment>
	</owl:Class>
	<owl:Class rdf:about="&j2se-1_3;OrgOmgCORBATypeCodePackageClassLibrary">
		<owl:equivalentClass rdf:resource="&j2se-1_2;OrgOmgCORBATypeCodePackageClassLibrary"/>
		<rdfs:subClassOf rdf:resource="&java;JavaClassLibrary"/>
		<rdfs:comment xml:lang="en">JavaLibrary implementing the org.omg.CORBA.TypeCodePackage package for J2SE 1.3</rdfs:comment>
		<rdfs:comment xml:lang="OWLManchester">platform:implementsInterface some OrgOmgCORBATypeCodePackageAPI</rdfs:comment>
	</owl:Class>
	<owl:Class rdf:about="&j2se-1_3;OrgOmgCORBAORBPackageClassLibrary">
		<owl:equivalentClass rdf:resource="&j2se-1_2;OrgOmgCORBAORBPackageClassLibrary"/>
		<rdfs:subClassOf rdf:resource="&java;JavaClassLibrary"/>
		<rdfs:comment xml:lang="en">JavaLibrary implementing the org.omg.CORBA.ORBPackage package for J2SE 1.3</rdfs:comment>
		<rdfs:comment xml:lang="OWLManchester">platform:implementsInterface some OrgOmgCORBAORBPackageAPI</rdfs:comment>
	</owl:Class>
	<owl:Class rdf:about="&j2se-1_3;OrgOmgCORBADynAnyPackageClassLibrary">
		<owl:equivalentClass rdf:resource="&j2se-1_2;OrgOmgCORBADynAnyPackageClassLibrary"/>
		<rdfs:subClassOf rdf:resource="&java;JavaClassLibrary"/>
		<rdfs:comment xml:lang="en">JavaLibrary implementing the org.omg.CORBA.DynAnyPackage package for J2SE 1.3</rdfs:comment>
		<rdfs:comment xml:lang="OWLManchester">platform:implementsInterface some OrgOmgCORBADynAnyPackageAPI</rdfs:comment>
	</owl:Class>
	<owl:Class rdf:about="&j2se-1_3;OrgOmgSendingContextClassLibrary">
		<rdfs:subClassOf rdf:resource="&java;JavaClassLibrary"/>
		<rdfs:comment xml:lang="en">JavaLibrary implementing the org.omg.SendingContext package for J2SE 1.3</rdfs:comment>
		<rdfs:comment xml:lang="OWLManchester">platform:implementsInterface some OrgOmgSendingContextAPI</rdfs:comment>
	</owl:Class>
	<owl:Class rdf:about="&j2se-1_3;OrgOmgCosNamingClassLibrary">
		<rdfs:subClassOf rdf:resource="&j2se-1_2;OrgOmgCosNamingClassLibrary"/>
		<rdfs:comment xml:lang="en">JavaLibrary implementing the org.omg.CosNaming package for J2SE 1.3</rdfs:comment>
		<rdfs:comment xml:lang="OWLManchester">platform:implementsInterface some OrgOmgCosNamingAPI</rdfs:comment>
	</owl:Class>
	<owl:Class rdf:about="&j2se-1_3;OrgOmgCosNamingNamingContextPackageClassLibrary">
		<owl:equivalentClass rdf:resource="&j2se-1_2;OrgOmgCosNamingNamingContextPackageClassLibrary"/>
		<rdfs:subClassOf rdf:resource="&java;JavaClassLibrary"/>
		<rdfs:comment xml:lang="en">JavaLibrary implementing the org.omg.CosNaming.NamingContextPackage package for J2SE 1.3</rdfs:comment>
		<rdfs:comment xml:lang="OWLManchester">platform:implementsInterface some OrgOmgCosNamingNamingContextPackageAPI</rdfs:comment>
	</owl:Class>
	<owl:Class rdf:about="&j2se-1_3;OrgOmgStubJavaRmiClassLibrary">
		<rdfs:subClassOf rdf:resource="&java;JavaClassLibrary"/>
		<rdfs:comment xml:lang="en">JavaLibrary implementing the org.omg.stub.java.rmi package for J2SE 1.3</rdfs:comment>
		<rdfs:comment xml:lang="OWLManchester">platform:implementsInterface some OrgOmgStubJavaRmiAPI</rdfs:comment>
	</owl:Class>
</rdf:RDF>
