<?xml version="1.0" encoding="ISO-8859-1"?>
<!DOCTYPE rdf:RDF [
	<!ENTITY platform "http://localhost/~dennis/platformkit/2010_1/platform.owl#">
	<!ENTITY xsd "http://www.w3.org/2001/XMLSchema#">
	<!ENTITY j2me-midp-2_0 "http://soft.vub.ac.be/platformkit/2010/1/j2me-midp-2_0.owl#">
	<!ENTITY j2se-1_2 "http://soft.vub.ac.be/platformkit/2010/1/j2se-1_2.owl#">
	<!ENTITY java "http://localhost/~dennis/platformkit/2010_1/java.owl#">
	<!ENTITY isa "http://localhost/~dennis/platformkit/2010_1/isa.owl#">
	<!ENTITY ns_19 "http://localhost/~dennis/platformkit/2010_1/">
	<!ENTITY jdk-1_1 "http://soft.vub.ac.be/platformkit/2010/1/jdk-1_1.owl#">
	<!ENTITY personaljava-1_1 "http://soft.vub.ac.be/platformkit/2010/1/personaljava-1_1.owl#">
	<!ENTITY rdf "http://www.w3.org/1999/02/22-rdf-syntax-ns#">
	<!ENTITY rdfs "http://www.w3.org/2000/01/rdf-schema#">
	<!ENTITY owl "http://www.w3.org/2002/07/owl#">
]>
<rdf:RDF
	 xmlns:platform="&platform;"
	 xmlns:xsd="&xsd;"
	 xmlns:j2me-midp-2_0="&j2me-midp-2_0;"
	 xmlns:j2se-1_2="&j2se-1_2;"
	 xmlns:java="&java;"
	 xmlns:isa="&isa;"
	 xmlns:ns_19="&ns_19;"
	 xmlns:jdk-1_1="&jdk-1_1;"
	 xmlns:personaljava-1_1="&personaljava-1_1;"
	 xmlns:rdf="&rdf;"
	 xmlns:rdfs="&rdfs;"
	 xmlns:owl="&owl;"
>

	<owl:Ontology rdf:about="http://soft.vub.ac.be/platformkit/2010/1/j2se-1_2.owl#">
		<owl:versionInfo>$Id: UML2ToPackageAPIOntology.atl 8082 2010-03-18 21:11:00Z dwagelaa $</owl:versionInfo>
		<owl:imports rdf:resource="http://localhost/~dennis/platformkit/2010_1/platform.owl"/>
		<owl:imports rdf:resource="http://localhost/~dennis/platformkit/2010_1/java.owl"/>
		<owl:imports rdf:resource="http://soft.vub.ac.be/platformkit/2010/1/j2me-midp-2_0.owl#"/>
		<owl:imports rdf:resource="http://soft.vub.ac.be/platformkit/2010/1/jdk-1_1.owl#"/>
		<owl:imports rdf:resource="http://soft.vub.ac.be/platformkit/2010/1/personaljava-1_1.owl#"/>
		<owl:imports rdf:resource="http://localhost/~dennis/platformkit/2010_1/isa.owl"/>
		<rdfs:comment xml:lang="en">Generated by [UML2ToSimplifiedPackageAPIOntology.atl 8080 2010-03-18 10:46:40Z dwagelaa], [UML2ToPackageAPIOntology.atl 8082 2010-03-18 21:11:00Z dwagelaa], [UML2ToAPIOntology.atl 8082 2010-03-18 21:11:00Z dwagelaa], and [UML2Comparison.atl 8082 2010-03-18 21:11:00Z dwagelaa]</rdfs:comment>
		<rdfs:comment>Dennis Wagelaar &lt;dennis.wagelaar@vub.ac.be&gt;</rdfs:comment>
		<rdfs:comment xml:lang="en">&#169; 2010, Vrije Universiteit Brussel. All rights reserved.</rdfs:comment>
		<rdfs:label xml:lang="en">J2SE 1.2</rdfs:label>
	</owl:Ontology>
	<owl:Class rdf:about="&j2se-1_2;J2SE1_2API">
		<rdfs:subClassOf rdf:resource="&j2se-1_2;JavaIoAPI"/>
		<rdfs:subClassOf rdf:resource="&j2se-1_2;JavaLangAPI"/>
		<rdfs:subClassOf rdf:resource="&j2se-1_2;JavaLangReflectAPI"/>
		<rdfs:subClassOf rdf:resource="&j2se-1_2;JavaLangRefAPI"/>
		<rdfs:subClassOf rdf:resource="&j2se-1_2;JavaNetAPI"/>
		<rdfs:subClassOf rdf:resource="&j2se-1_2;JavaSecurityAPI"/>
		<rdfs:subClassOf rdf:resource="&j2se-1_2;JavaSecurityCertAPI"/>
		<rdfs:subClassOf rdf:resource="&j2se-1_2;JavaSecuritySpecAPI"/>
		<rdfs:subClassOf rdf:resource="&j2se-1_2;JavaSecurityInterfacesAPI"/>
		<rdfs:subClassOf rdf:resource="&j2se-1_2;JavaSecurityAclAPI"/>
		<rdfs:subClassOf rdf:resource="&j2se-1_2;JavaUtilAPI"/>
		<rdfs:subClassOf rdf:resource="&j2se-1_2;JavaUtilJarAPI"/>
		<rdfs:subClassOf rdf:resource="&j2se-1_2;JavaUtilZipAPI"/>
		<rdfs:subClassOf rdf:resource="&j2se-1_2;JavaMathAPI"/>
		<rdfs:subClassOf rdf:resource="&j2se-1_2;JavaTextAPI"/>
		<rdfs:subClassOf rdf:resource="&j2se-1_2;JavaTextResourcesAPI"/>
		<rdfs:subClassOf rdf:resource="&j2se-1_2;JavaAwtAPI"/>
		<rdfs:subClassOf rdf:resource="&j2se-1_2;JavaAwtGeomAPI"/>
		<rdfs:subClassOf rdf:resource="&j2se-1_2;JavaAwtImageAPI"/>
		<rdfs:subClassOf rdf:resource="&j2se-1_2;JavaAwtImageRenderableAPI"/>
		<rdfs:subClassOf rdf:resource="&j2se-1_2;JavaAwtFontAPI"/>
		<rdfs:subClassOf rdf:resource="&j2se-1_2;JavaAwtEventAPI"/>
		<rdfs:subClassOf rdf:resource="&j2se-1_2;JavaAwtDndAPI"/>
		<rdfs:subClassOf rdf:resource="&j2se-1_2;JavaAwtDatatransferAPI"/>
		<rdfs:subClassOf rdf:resource="&j2se-1_2;JavaAwtImAPI"/>
		<rdfs:subClassOf rdf:resource="&j2se-1_2;JavaAwtPrintAPI"/>
		<rdfs:subClassOf rdf:resource="&j2se-1_2;JavaAwtColorAPI"/>
		<rdfs:subClassOf rdf:resource="&j2se-1_2;JavaBeansAPI"/>
		<rdfs:subClassOf rdf:resource="&j2se-1_2;JavaBeansBeancontextAPI"/>
		<rdfs:subClassOf rdf:resource="&j2se-1_2;JavaAppletAPI"/>
		<rdfs:subClassOf rdf:resource="&j2se-1_2;JavaRmiAPI"/>
		<rdfs:subClassOf rdf:resource="&j2se-1_2;JavaRmiServerAPI"/>
		<rdfs:subClassOf rdf:resource="&j2se-1_2;JavaRmiDgcAPI"/>
		<rdfs:subClassOf rdf:resource="&j2se-1_2;JavaRmiRegistryAPI"/>
		<rdfs:subClassOf rdf:resource="&j2se-1_2;JavaRmiActivationAPI"/>
		<rdfs:subClassOf rdf:resource="&j2se-1_2;JavaSqlAPI"/>
		<rdfs:subClassOf rdf:resource="&j2se-1_2;JavaxSwingAPI"/>
		<rdfs:subClassOf rdf:resource="&j2se-1_2;JavaxSwingEventAPI"/>
		<rdfs:subClassOf rdf:resource="&j2se-1_2;JavaxSwingTextAPI"/>
		<rdfs:subClassOf rdf:resource="&j2se-1_2;JavaxSwingTextHtmlAPI"/>
		<rdfs:subClassOf rdf:resource="&j2se-1_2;JavaxSwingTextHtmlParserAPI"/>
		<rdfs:subClassOf rdf:resource="&j2se-1_2;JavaxSwingTextRtfAPI"/>
		<rdfs:subClassOf rdf:resource="&j2se-1_2;JavaxSwingUndoAPI"/>
		<rdfs:subClassOf rdf:resource="&j2se-1_2;JavaxSwingTableAPI"/>
		<rdfs:subClassOf rdf:resource="&j2se-1_2;JavaxSwingTreeAPI"/>
		<rdfs:subClassOf rdf:resource="&j2se-1_2;JavaxSwingPlafAPI"/>
		<rdfs:subClassOf rdf:resource="&j2se-1_2;JavaxSwingPlafBasicAPI"/>
		<rdfs:subClassOf rdf:resource="&j2se-1_2;JavaxSwingPlafMetalAPI"/>
		<rdfs:subClassOf rdf:resource="&j2se-1_2;JavaxSwingPlafMultiAPI"/>
		<rdfs:subClassOf rdf:resource="&j2se-1_2;JavaxSwingBorderAPI"/>
		<rdfs:subClassOf rdf:resource="&j2se-1_2;JavaxSwingColorchooserAPI"/>
		<rdfs:subClassOf rdf:resource="&j2se-1_2;JavaxSwingFilechooserAPI"/>
		<rdfs:subClassOf rdf:resource="&j2se-1_2;JavaxAccessibilityAPI"/>
		<rdfs:subClassOf rdf:resource="&j2se-1_2;OrgOmgCORBAAPI"/>
		<rdfs:subClassOf rdf:resource="&j2se-1_2;OrgOmgCORBAPortableAPI"/>
		<rdfs:subClassOf rdf:resource="&j2se-1_2;OrgOmgCORBADynAnyPackageAPI"/>
		<rdfs:subClassOf rdf:resource="&j2se-1_2;OrgOmgCORBAORBPackageAPI"/>
		<rdfs:subClassOf rdf:resource="&j2se-1_2;OrgOmgCORBATypeCodePackageAPI"/>
		<rdfs:subClassOf rdf:resource="&j2se-1_2;OrgOmgCosNamingAPI"/>
		<rdfs:subClassOf rdf:resource="&j2se-1_2;OrgOmgCosNamingNamingContextPackageAPI"/>
		<rdfs:comment xml:lang="en">J2SE 1.2 API</rdfs:comment>
		<rdfs:comment xml:lang="OWLManchester">platform:comprisesInterfacePart some JavaIo and platform:comprisesInterfacePart some JavaLang and platform:comprisesInterfacePart some JavaLangReflect and platform:comprisesInterfacePart some JavaLangRef and platform:comprisesInterfacePart some JavaNet and platform:comprisesInterfacePart some JavaSecurity and platform:comprisesInterfacePart some JavaSecurityCert and platform:comprisesInterfacePart some JavaSecuritySpec and platform:comprisesInterfacePart some JavaSecurityInterfaces and platform:comprisesInterfacePart some JavaSecurityAcl and platform:comprisesInterfacePart some JavaUtil and platform:comprisesInterfacePart some JavaUtilJar and platform:comprisesInterfacePart some JavaUtilZip and platform:comprisesInterfacePart some JavaMath and platform:comprisesInterfacePart some JavaText and platform:comprisesInterfacePart some JavaTextResources and platform:comprisesInterfacePart some JavaAwt and platform:comprisesInterfacePart some JavaAwtGeom and platform:comprisesInterfacePart some JavaAwtImage and platform:comprisesInterfacePart some JavaAwtImageRenderable and platform:comprisesInterfacePart some JavaAwtFont and platform:comprisesInterfacePart some JavaAwtEvent and platform:comprisesInterfacePart some JavaAwtDnd and platform:comprisesInterfacePart some JavaAwtDatatransfer and platform:comprisesInterfacePart some JavaAwtIm and platform:comprisesInterfacePart some JavaAwtPrint and platform:comprisesInterfacePart some JavaAwtColor and platform:comprisesInterfacePart some JavaBeans and platform:comprisesInterfacePart some JavaBeansBeancontext and platform:comprisesInterfacePart some JavaApplet and platform:comprisesInterfacePart some JavaRmi and platform:comprisesInterfacePart some JavaRmiServer and platform:comprisesInterfacePart some JavaRmiDgc and platform:comprisesInterfacePart some JavaRmiRegistry and platform:comprisesInterfacePart some JavaRmiActivation and platform:comprisesInterfacePart some JavaSql and platform:comprisesInterfacePart some JavaxSwing and platform:comprisesInterfacePart some JavaxSwingEvent and platform:comprisesInterfacePart some JavaxSwingText and platform:comprisesInterfacePart some JavaxSwingTextHtml and platform:comprisesInterfacePart some JavaxSwingTextHtmlParser and platform:comprisesInterfacePart some JavaxSwingTextRtf and platform:comprisesInterfacePart some JavaxSwingUndo and platform:comprisesInterfacePart some JavaxSwingTable and platform:comprisesInterfacePart some JavaxSwingTree and platform:comprisesInterfacePart some JavaxSwingPlaf and platform:comprisesInterfacePart some JavaxSwingPlafBasic and platform:comprisesInterfacePart some JavaxSwingPlafMetal and platform:comprisesInterfacePart some JavaxSwingPlafMulti and platform:comprisesInterfacePart some JavaxSwingBorder and platform:comprisesInterfacePart some JavaxSwingColorchooser and platform:comprisesInterfacePart some JavaxSwingFilechooser and platform:comprisesInterfacePart some JavaxAccessibility and platform:comprisesInterfacePart some OrgOmgCORBA and platform:comprisesInterfacePart some OrgOmgCORBAPortable and platform:comprisesInterfacePart some OrgOmgCORBADynAnyPackage and platform:comprisesInterfacePart some OrgOmgCORBAORBPackage and platform:comprisesInterfacePart some OrgOmgCORBATypeCodePackage and platform:comprisesInterfacePart some OrgOmgCosNaming and platform:comprisesInterfacePart some OrgOmgCosNamingNamingContextPackage</rdfs:comment>
	</owl:Class>
	<owl:Class rdf:about="&j2se-1_2;J2SE1_2ClassLibrary">
		<rdfs:subClassOf rdf:resource="&j2se-1_2;JavaIoClassLibrary"/>
		<rdfs:subClassOf rdf:resource="&j2se-1_2;JavaLangClassLibrary"/>
		<rdfs:subClassOf rdf:resource="&j2se-1_2;JavaLangReflectClassLibrary"/>
		<rdfs:subClassOf rdf:resource="&j2se-1_2;JavaLangRefClassLibrary"/>
		<rdfs:subClassOf rdf:resource="&j2se-1_2;JavaNetClassLibrary"/>
		<rdfs:subClassOf rdf:resource="&j2se-1_2;JavaSecurityClassLibrary"/>
		<rdfs:subClassOf rdf:resource="&j2se-1_2;JavaSecurityCertClassLibrary"/>
		<rdfs:subClassOf rdf:resource="&j2se-1_2;JavaSecuritySpecClassLibrary"/>
		<rdfs:subClassOf rdf:resource="&j2se-1_2;JavaSecurityInterfacesClassLibrary"/>
		<rdfs:subClassOf rdf:resource="&j2se-1_2;JavaSecurityAclClassLibrary"/>
		<rdfs:subClassOf rdf:resource="&j2se-1_2;JavaUtilClassLibrary"/>
		<rdfs:subClassOf rdf:resource="&j2se-1_2;JavaUtilJarClassLibrary"/>
		<rdfs:subClassOf rdf:resource="&j2se-1_2;JavaUtilZipClassLibrary"/>
		<rdfs:subClassOf rdf:resource="&j2se-1_2;JavaMathClassLibrary"/>
		<rdfs:subClassOf rdf:resource="&j2se-1_2;JavaTextClassLibrary"/>
		<rdfs:subClassOf rdf:resource="&j2se-1_2;JavaTextResourcesClassLibrary"/>
		<rdfs:subClassOf rdf:resource="&j2se-1_2;JavaAwtClassLibrary"/>
		<rdfs:subClassOf rdf:resource="&j2se-1_2;JavaAwtGeomClassLibrary"/>
		<rdfs:subClassOf rdf:resource="&j2se-1_2;JavaAwtImageClassLibrary"/>
		<rdfs:subClassOf rdf:resource="&j2se-1_2;JavaAwtImageRenderableClassLibrary"/>
		<rdfs:subClassOf rdf:resource="&j2se-1_2;JavaAwtFontClassLibrary"/>
		<rdfs:subClassOf rdf:resource="&j2se-1_2;JavaAwtEventClassLibrary"/>
		<rdfs:subClassOf rdf:resource="&j2se-1_2;JavaAwtDndClassLibrary"/>
		<rdfs:subClassOf rdf:resource="&j2se-1_2;JavaAwtDatatransferClassLibrary"/>
		<rdfs:subClassOf rdf:resource="&j2se-1_2;JavaAwtImClassLibrary"/>
		<rdfs:subClassOf rdf:resource="&j2se-1_2;JavaAwtPrintClassLibrary"/>
		<rdfs:subClassOf rdf:resource="&j2se-1_2;JavaAwtColorClassLibrary"/>
		<rdfs:subClassOf rdf:resource="&j2se-1_2;JavaBeansClassLibrary"/>
		<rdfs:subClassOf rdf:resource="&j2se-1_2;JavaBeansBeancontextClassLibrary"/>
		<rdfs:subClassOf rdf:resource="&j2se-1_2;JavaAppletClassLibrary"/>
		<rdfs:subClassOf rdf:resource="&j2se-1_2;JavaRmiClassLibrary"/>
		<rdfs:subClassOf rdf:resource="&j2se-1_2;JavaRmiServerClassLibrary"/>
		<rdfs:subClassOf rdf:resource="&j2se-1_2;JavaRmiDgcClassLibrary"/>
		<rdfs:subClassOf rdf:resource="&j2se-1_2;JavaRmiRegistryClassLibrary"/>
		<rdfs:subClassOf rdf:resource="&j2se-1_2;JavaRmiActivationClassLibrary"/>
		<rdfs:subClassOf rdf:resource="&j2se-1_2;JavaSqlClassLibrary"/>
		<rdfs:subClassOf rdf:resource="&j2se-1_2;JavaxSwingClassLibrary"/>
		<rdfs:subClassOf rdf:resource="&j2se-1_2;JavaxSwingEventClassLibrary"/>
		<rdfs:subClassOf rdf:resource="&j2se-1_2;JavaxSwingTextClassLibrary"/>
		<rdfs:subClassOf rdf:resource="&j2se-1_2;JavaxSwingTextHtmlClassLibrary"/>
		<rdfs:subClassOf rdf:resource="&j2se-1_2;JavaxSwingTextHtmlParserClassLibrary"/>
		<rdfs:subClassOf rdf:resource="&j2se-1_2;JavaxSwingTextRtfClassLibrary"/>
		<rdfs:subClassOf rdf:resource="&j2se-1_2;JavaxSwingUndoClassLibrary"/>
		<rdfs:subClassOf rdf:resource="&j2se-1_2;JavaxSwingTableClassLibrary"/>
		<rdfs:subClassOf rdf:resource="&j2se-1_2;JavaxSwingTreeClassLibrary"/>
		<rdfs:subClassOf rdf:resource="&j2se-1_2;JavaxSwingPlafClassLibrary"/>
		<rdfs:subClassOf rdf:resource="&j2se-1_2;JavaxSwingPlafBasicClassLibrary"/>
		<rdfs:subClassOf rdf:resource="&j2se-1_2;JavaxSwingPlafMetalClassLibrary"/>
		<rdfs:subClassOf rdf:resource="&j2se-1_2;JavaxSwingPlafMultiClassLibrary"/>
		<rdfs:subClassOf rdf:resource="&j2se-1_2;JavaxSwingBorderClassLibrary"/>
		<rdfs:subClassOf rdf:resource="&j2se-1_2;JavaxSwingColorchooserClassLibrary"/>
		<rdfs:subClassOf rdf:resource="&j2se-1_2;JavaxSwingFilechooserClassLibrary"/>
		<rdfs:subClassOf rdf:resource="&j2se-1_2;JavaxAccessibilityClassLibrary"/>
		<rdfs:subClassOf rdf:resource="&j2se-1_2;OrgOmgCORBAClassLibrary"/>
		<rdfs:subClassOf rdf:resource="&j2se-1_2;OrgOmgCORBAPortableClassLibrary"/>
		<rdfs:subClassOf rdf:resource="&j2se-1_2;OrgOmgCORBADynAnyPackageClassLibrary"/>
		<rdfs:subClassOf rdf:resource="&j2se-1_2;OrgOmgCORBAORBPackageClassLibrary"/>
		<rdfs:subClassOf rdf:resource="&j2se-1_2;OrgOmgCORBATypeCodePackageClassLibrary"/>
		<rdfs:subClassOf rdf:resource="&j2se-1_2;OrgOmgCosNamingClassLibrary"/>
		<rdfs:subClassOf rdf:resource="&j2se-1_2;OrgOmgCosNamingNamingContextPackageClassLibrary"/>
		<rdfs:comment xml:lang="en">Java class library implementing the J2SE 1.2 API</rdfs:comment>
		<rdfs:comment xml:lang="OWLManchester">platform:implementsInterface some J2SE1_2API</rdfs:comment>
	</owl:Class>
	<owl:Class rdf:about="&j2se-1_2;J2SE1_2BytecodeFormat">
		<rdfs:subClassOf rdf:resource="&jdk-1_1;JDK1_1BytecodeFormat"/>
		<rdfs:subClassOf rdf:resource="&personaljava-1_1;PersonalJava1_1BytecodeFormat"/>
		<rdfs:comment xml:lang="en">J2SE 1.2 bytecode format</rdfs:comment>
		<rdfs:comment xml:lang="OWLManchester">java:majorVersionNumber some xsd:integer[>="46"^^xsd:integer] and java:preverified value false</rdfs:comment>
	</owl:Class>
	<j2se-1_2:J2SE1_2BytecodeFormat rdf:about="&j2se-1_2;theJ2SE1_2BytecodeFormat">
		<java:preverified rdf:datatype="http://www.w3.org/2001/XMLSchema#boolean">false</java:preverified>
		<java:minorVersionNumber rdf:datatype="http://www.w3.org/2001/XMLSchema#integer">0</java:minorVersionNumber>
		<java:majorVersionNumber rdf:datatype="http://www.w3.org/2001/XMLSchema#integer">46</java:majorVersionNumber>
	</j2se-1_2:J2SE1_2BytecodeFormat>
	<j2se-1_2:J2SE1_2API rdf:about="&j2se-1_2;theJ2SE1_2API">
		<platform:comprisesInterfacePart rdf:resource="&j2se-1_2;theOrgOmgCosNamingNamingContextPackagePart"/>
		<platform:comprisesInterfacePart rdf:resource="&j2se-1_2;theOrgOmgCosNamingPart"/>
		<platform:comprisesInterfacePart rdf:resource="&j2se-1_2;theOrgOmgCORBATypeCodePackagePart"/>
		<platform:comprisesInterfacePart rdf:resource="&j2se-1_2;theOrgOmgCORBAORBPackagePart"/>
		<platform:comprisesInterfacePart rdf:resource="&j2se-1_2;theOrgOmgCORBADynAnyPackagePart"/>
		<platform:comprisesInterfacePart rdf:resource="&j2se-1_2;theOrgOmgCORBAPortablePart"/>
		<platform:comprisesInterfacePart rdf:resource="&j2se-1_2;theOrgOmgCORBAPart"/>
		<platform:comprisesInterfacePart rdf:resource="&j2se-1_2;theJavaxAccessibilityPart"/>
		<platform:comprisesInterfacePart rdf:resource="&j2se-1_2;theJavaxSwingFilechooserPart"/>
		<platform:comprisesInterfacePart rdf:resource="&j2se-1_2;theJavaxSwingColorchooserPart"/>
		<platform:comprisesInterfacePart rdf:resource="&j2se-1_2;theJavaxSwingBorderPart"/>
		<platform:comprisesInterfacePart rdf:resource="&j2se-1_2;theJavaxSwingPlafMultiPart"/>
		<platform:comprisesInterfacePart rdf:resource="&j2se-1_2;theJavaxSwingPlafMetalPart"/>
		<platform:comprisesInterfacePart rdf:resource="&j2se-1_2;theJavaxSwingPlafBasicPart"/>
		<platform:comprisesInterfacePart rdf:resource="&j2se-1_2;theJavaxSwingPlafPart"/>
		<platform:comprisesInterfacePart rdf:resource="&j2se-1_2;theJavaxSwingTreePart"/>
		<platform:comprisesInterfacePart rdf:resource="&j2se-1_2;theJavaxSwingTablePart"/>
		<platform:comprisesInterfacePart rdf:resource="&j2se-1_2;theJavaxSwingUndoPart"/>
		<platform:comprisesInterfacePart rdf:resource="&j2se-1_2;theJavaxSwingTextRtfPart"/>
		<platform:comprisesInterfacePart rdf:resource="&j2se-1_2;theJavaxSwingTextHtmlParserPart"/>
		<platform:comprisesInterfacePart rdf:resource="&j2se-1_2;theJavaxSwingTextHtmlPart"/>
		<platform:comprisesInterfacePart rdf:resource="&j2se-1_2;theJavaxSwingTextPart"/>
		<platform:comprisesInterfacePart rdf:resource="&j2se-1_2;theJavaxSwingEventPart"/>
		<platform:comprisesInterfacePart rdf:resource="&j2se-1_2;theJavaxSwingPart"/>
		<platform:comprisesInterfacePart rdf:resource="&j2se-1_2;theJavaSqlPart"/>
		<platform:comprisesInterfacePart rdf:resource="&j2se-1_2;theJavaRmiActivationPart"/>
		<platform:comprisesInterfacePart rdf:resource="&j2se-1_2;theJavaRmiRegistryPart"/>
		<platform:comprisesInterfacePart rdf:resource="&j2se-1_2;theJavaRmiDgcPart"/>
		<platform:comprisesInterfacePart rdf:resource="&j2se-1_2;theJavaRmiServerPart"/>
		<platform:comprisesInterfacePart rdf:resource="&j2se-1_2;theJavaRmiPart"/>
		<platform:comprisesInterfacePart rdf:resource="&j2se-1_2;theJavaAppletPart"/>
		<platform:comprisesInterfacePart rdf:resource="&j2se-1_2;theJavaBeansBeancontextPart"/>
		<platform:comprisesInterfacePart rdf:resource="&j2se-1_2;theJavaBeansPart"/>
		<platform:comprisesInterfacePart rdf:resource="&j2se-1_2;theJavaAwtColorPart"/>
		<platform:comprisesInterfacePart rdf:resource="&j2se-1_2;theJavaAwtPrintPart"/>
		<platform:comprisesInterfacePart rdf:resource="&j2se-1_2;theJavaAwtImPart"/>
		<platform:comprisesInterfacePart rdf:resource="&j2se-1_2;theJavaAwtDatatransferPart"/>
		<platform:comprisesInterfacePart rdf:resource="&j2se-1_2;theJavaAwtDndPart"/>
		<platform:comprisesInterfacePart rdf:resource="&j2se-1_2;theJavaAwtEventPart"/>
		<platform:comprisesInterfacePart rdf:resource="&j2se-1_2;theJavaAwtFontPart"/>
		<platform:comprisesInterfacePart rdf:resource="&j2se-1_2;theJavaAwtImageRenderablePart"/>
		<platform:comprisesInterfacePart rdf:resource="&j2se-1_2;theJavaAwtImagePart"/>
		<platform:comprisesInterfacePart rdf:resource="&j2se-1_2;theJavaAwtGeomPart"/>
		<platform:comprisesInterfacePart rdf:resource="&j2se-1_2;theJavaAwtPart"/>
		<platform:comprisesInterfacePart rdf:resource="&j2se-1_2;theJavaTextResourcesPart"/>
		<platform:comprisesInterfacePart rdf:resource="&j2se-1_2;theJavaTextPart"/>
		<platform:comprisesInterfacePart rdf:resource="&j2se-1_2;theJavaMathPart"/>
		<platform:comprisesInterfacePart rdf:resource="&j2se-1_2;theJavaUtilZipPart"/>
		<platform:comprisesInterfacePart rdf:resource="&j2se-1_2;theJavaUtilJarPart"/>
		<platform:comprisesInterfacePart rdf:resource="&j2se-1_2;theJavaUtilPart"/>
		<platform:comprisesInterfacePart rdf:resource="&j2se-1_2;theJavaSecurityAclPart"/>
		<platform:comprisesInterfacePart rdf:resource="&j2se-1_2;theJavaSecurityInterfacesPart"/>
		<platform:comprisesInterfacePart rdf:resource="&j2se-1_2;theJavaSecuritySpecPart"/>
		<platform:comprisesInterfacePart rdf:resource="&j2se-1_2;theJavaSecurityCertPart"/>
		<platform:comprisesInterfacePart rdf:resource="&j2se-1_2;theJavaSecurityPart"/>
		<platform:comprisesInterfacePart rdf:resource="&j2se-1_2;theJavaNetPart"/>
		<platform:comprisesInterfacePart rdf:resource="&j2se-1_2;theJavaLangRefPart"/>
		<platform:comprisesInterfacePart rdf:resource="&j2se-1_2;theJavaLangReflectPart"/>
		<platform:comprisesInterfacePart rdf:resource="&j2se-1_2;theJavaLangPart"/>
		<platform:comprisesInterfacePart rdf:resource="&j2se-1_2;theJavaIoPart"/>
	</j2se-1_2:J2SE1_2API>
	<owl:Class rdf:about="&j2se-1_2;J2SE1_2VM">
		<owl:equivalentClass>
			<owl:Restriction>
				<owl:onProperty rdf:resource="&platform;implementsInterface"/>
				<owl:someValuesFrom rdf:resource="&j2se-1_2;J2SE1_2BytecodeFormat"/>
			</owl:Restriction>
		</owl:equivalentClass>
		<rdfs:subClassOf rdf:resource="&java;JavaVM"/>
		<rdfs:comment xml:lang="en">J2SE 1.2 virtual machine</rdfs:comment>
	</owl:Class>
	<owl:Class rdf:about="&j2se-1_2;J2SE1_2JRE">
		<owl:equivalentClass>
			<owl:Class >
				<owl:intersectionOf rdf:parseType="Collection">
					<owl:Restriction>
						<owl:onProperty rdf:resource="&platform;providesFeature"/>
						<owl:someValuesFrom rdf:resource="&j2se-1_2;J2SE1_2ClassLibrary"/>
					</owl:Restriction>
					<owl:Restriction>
						<owl:onProperty rdf:resource="&platform;providesFeature"/>
						<owl:someValuesFrom rdf:resource="&j2se-1_2;J2SE1_2VM"/>
					</owl:Restriction>
				</owl:intersectionOf>
			</owl:Class>
		</owl:equivalentClass>
		<rdfs:subClassOf rdf:resource="&java;JRE"/>
		<rdfs:comment xml:lang="en">J2SE 1.2 Java Runtime Environment</rdfs:comment>
	</owl:Class>
	<owl:Class rdf:about="&j2se-1_2;JavaIo">
		<rdfs:subClassOf rdf:resource="&jdk-1_1;JavaIo"/>
		<rdfs:subClassOf rdf:resource="&j2me-midp-2_0;JavaIo"/>
		<rdfs:subClassOf rdf:resource="&personaljava-1_1;JavaIo"/>
		<rdfs:seeAlso rdf:resource="&j2se-1_2;JavaSecurity"/>
		<rdfs:seeAlso rdf:resource="&j2se-1_2;JavaNet"/>
		<rdfs:seeAlso rdf:resource="&j2se-1_2;JavaLang"/>
		<rdfs:seeAlso rdf:resource="&j2se-1_2;JavaUtil"/>
		<rdfs:comment xml:lang="en">Java API part implementing the java.io package for J2SE 1.2</rdfs:comment>
	</owl:Class>
	<owl:Class rdf:about="&j2se-1_2;JavaLang">
		<rdfs:subClassOf rdf:resource="&j2me-midp-2_0;JavaLang"/>
		<rdfs:seeAlso rdf:resource="&j2se-1_2;JavaSecurity"/>
		<rdfs:seeAlso rdf:resource="&j2se-1_2;JavaLangReflect"/>
		<rdfs:seeAlso rdf:resource="&j2se-1_2;JavaNet"/>
		<rdfs:seeAlso rdf:resource="&j2se-1_2;JavaIo"/>
		<rdfs:seeAlso rdf:resource="&j2se-1_2;JavaUtil"/>
		<rdfs:comment xml:lang="en">Java API part implementing the java.lang package for J2SE 1.2</rdfs:comment>
	</owl:Class>
	<owl:Class rdf:about="&j2se-1_2;JavaLangReflect">
		<rdfs:subClassOf rdf:resource="&jdk-1_1;JavaLangReflect"/>
		<rdfs:subClassOf rdf:resource="&personaljava-1_1;JavaLangReflect"/>
		<rdfs:seeAlso rdf:resource="&j2se-1_2;JavaSecurity"/>
		<rdfs:seeAlso rdf:resource="&j2se-1_2;JavaLang"/>
		<rdfs:seeAlso rdf:resource="&j2se-1_2;JavaIo"/>
		<rdfs:comment xml:lang="en">Java API part implementing the java.lang.reflect package for J2SE 1.2</rdfs:comment>
	</owl:Class>
	<owl:Class rdf:about="&j2se-1_2;JavaLangRef">
		<rdfs:subClassOf rdf:resource="&java;JavaAPIPart"/>
		<rdfs:seeAlso rdf:resource="&j2se-1_2;JavaLang"/>
		<rdfs:comment xml:lang="en">Java API part implementing the java.lang.ref package for J2SE 1.2</rdfs:comment>
	</owl:Class>
	<owl:Class rdf:about="&j2se-1_2;JavaNet">
		<rdfs:subClassOf rdf:resource="&jdk-1_1;JavaNet"/>
		<rdfs:subClassOf rdf:resource="&personaljava-1_1;JavaNet"/>
		<rdfs:seeAlso rdf:resource="&j2se-1_2;JavaSecurity"/>
		<rdfs:seeAlso rdf:resource="&j2se-1_2;JavaLang"/>
		<rdfs:seeAlso rdf:resource="&j2se-1_2;JavaUtilJar"/>
		<rdfs:seeAlso rdf:resource="&j2se-1_2;JavaIo"/>
		<rdfs:seeAlso rdf:resource="&j2se-1_2;JavaUtil"/>
		<rdfs:comment xml:lang="en">Java API part implementing the java.net package for J2SE 1.2</rdfs:comment>
	</owl:Class>
	<owl:Class rdf:about="&j2se-1_2;JavaSecurity">
		<rdfs:subClassOf rdf:resource="&jdk-1_1;JavaSecurity"/>
		<rdfs:seeAlso rdf:resource="&j2se-1_2;JavaSecurityCert"/>
		<rdfs:seeAlso rdf:resource="&j2se-1_2;JavaSecuritySpec"/>
		<rdfs:seeAlso rdf:resource="&j2se-1_2;JavaNet"/>
		<rdfs:seeAlso rdf:resource="&j2se-1_2;JavaIo"/>
		<rdfs:seeAlso rdf:resource="&j2se-1_2;JavaUtil"/>
		<rdfs:seeAlso rdf:resource="&j2se-1_2;JavaLang"/>
		<rdfs:comment xml:lang="en">Java API part implementing the java.security package for J2SE 1.2</rdfs:comment>
	</owl:Class>
	<owl:Class rdf:about="&j2se-1_2;JavaSecurityCert">
		<rdfs:subClassOf rdf:resource="&java;JavaAPIPart"/>
		<rdfs:seeAlso rdf:resource="&j2se-1_2;JavaSecurity"/>
		<rdfs:seeAlso rdf:resource="&j2se-1_2;JavaMath"/>
		<rdfs:seeAlso rdf:resource="&j2se-1_2;JavaLang"/>
		<rdfs:seeAlso rdf:resource="&j2se-1_2;JavaIo"/>
		<rdfs:seeAlso rdf:resource="&j2se-1_2;JavaUtil"/>
		<rdfs:comment xml:lang="en">Java API part implementing the java.security.cert package for J2SE 1.2</rdfs:comment>
	</owl:Class>
	<owl:Class rdf:about="&j2se-1_2;JavaSecuritySpec">
		<rdfs:subClassOf rdf:resource="&java;JavaAPIPart"/>
		<rdfs:seeAlso rdf:resource="&j2se-1_2;JavaSecurity"/>
		<rdfs:seeAlso rdf:resource="&j2se-1_2;JavaMath"/>
		<rdfs:seeAlso rdf:resource="&j2se-1_2;JavaLang"/>
		<rdfs:seeAlso rdf:resource="&j2se-1_2;JavaSecurityInterfaces"/>
		<rdfs:comment xml:lang="en">Java API part implementing the java.security.spec package for J2SE 1.2</rdfs:comment>
	</owl:Class>
	<owl:Class rdf:about="&j2se-1_2;JavaSecurityInterfaces">
		<rdfs:subClassOf rdf:resource="&jdk-1_1;JavaSecurityInterfaces"/>
		<rdfs:seeAlso rdf:resource="&j2se-1_2;JavaSecurity"/>
		<rdfs:seeAlso rdf:resource="&j2se-1_2;JavaMath"/>
		<rdfs:comment xml:lang="en">Java API part implementing the java.security.interfaces package for J2SE 1.2</rdfs:comment>
	</owl:Class>
	<owl:Class rdf:about="&j2se-1_2;JavaSecurityAcl">
		<owl:equivalentClass rdf:resource="&jdk-1_1;JavaSecurityAcl"/>
		<rdfs:subClassOf rdf:resource="&java;JavaAPIPart"/>
		<rdfs:seeAlso rdf:resource="&j2se-1_2;JavaSecurity"/>
		<rdfs:seeAlso rdf:resource="&j2se-1_2;JavaLang"/>
		<rdfs:seeAlso rdf:resource="&j2se-1_2;JavaUtil"/>
		<rdfs:comment xml:lang="en">Java API part implementing the java.security.acl package for J2SE 1.2</rdfs:comment>
	</owl:Class>
	<owl:Class rdf:about="&j2se-1_2;JavaUtil">
		<rdfs:subClassOf rdf:resource="&jdk-1_1;JavaUtil"/>
		<rdfs:subClassOf rdf:resource="&personaljava-1_1;JavaUtil"/>
		<rdfs:seeAlso rdf:resource="&j2se-1_2;JavaSecurity"/>
		<rdfs:seeAlso rdf:resource="&j2se-1_2;JavaLang"/>
		<rdfs:seeAlso rdf:resource="&j2se-1_2;JavaIo"/>
		<rdfs:comment xml:lang="en">Java API part implementing the java.util package for J2SE 1.2</rdfs:comment>
	</owl:Class>
	<owl:Class rdf:about="&j2se-1_2;JavaUtilJar">
		<rdfs:subClassOf rdf:resource="&java;JavaAPIPart"/>
		<rdfs:seeAlso rdf:resource="&j2se-1_2;JavaLang"/>
		<rdfs:seeAlso rdf:resource="&j2se-1_2;JavaUtilZip"/>
		<rdfs:seeAlso rdf:resource="&j2se-1_2;JavaIo"/>
		<rdfs:seeAlso rdf:resource="&j2se-1_2;JavaUtil"/>
		<rdfs:comment xml:lang="en">Java API part implementing the java.util.jar package for J2SE 1.2</rdfs:comment>
	</owl:Class>
	<owl:Class rdf:about="&j2se-1_2;JavaUtilZip">
		<rdfs:subClassOf rdf:resource="&jdk-1_1;JavaUtilZip"/>
		<rdfs:subClassOf rdf:resource="&personaljava-1_1;JavaUtilZip"/>
		<rdfs:seeAlso rdf:resource="&j2se-1_2;JavaLang"/>
		<rdfs:seeAlso rdf:resource="&j2se-1_2;JavaIo"/>
		<rdfs:seeAlso rdf:resource="&j2se-1_2;JavaUtil"/>
		<rdfs:comment xml:lang="en">Java API part implementing the java.util.zip package for J2SE 1.2</rdfs:comment>
	</owl:Class>
	<owl:Class rdf:about="&j2se-1_2;JavaMath">
		<rdfs:subClassOf rdf:resource="&jdk-1_1;JavaMath"/>
		<rdfs:seeAlso rdf:resource="&j2se-1_2;JavaLang"/>
		<rdfs:seeAlso rdf:resource="&j2se-1_2;JavaUtil"/>
		<rdfs:comment xml:lang="en">Java API part implementing the java.math package for J2SE 1.2</rdfs:comment>
	</owl:Class>
	<owl:Class rdf:about="&j2se-1_2;JavaText">
		<rdfs:subClassOf rdf:resource="&java;JavaAPIPart"/>
		<rdfs:seeAlso rdf:resource="&j2se-1_2;JavaLang"/>
		<rdfs:seeAlso rdf:resource="&j2se-1_2;JavaIo"/>
		<rdfs:seeAlso rdf:resource="&j2se-1_2;JavaUtil"/>
		<rdfs:comment xml:lang="en">Java API part implementing the java.text package for J2SE 1.2</rdfs:comment>
	</owl:Class>
	<owl:Class rdf:about="&j2se-1_2;JavaTextResources">
		<rdfs:subClassOf rdf:resource="&personaljava-1_1;JavaTextResources"/>
		<rdfs:seeAlso rdf:resource="&j2se-1_2;JavaLang"/>
		<rdfs:seeAlso rdf:resource="&j2se-1_2;JavaUtil"/>
		<rdfs:comment xml:lang="en">Java API part implementing the java.text.resources package for J2SE 1.2</rdfs:comment>
	</owl:Class>
	<owl:Class rdf:about="&j2se-1_2;JavaAwt">
		<rdfs:subClassOf rdf:resource="&jdk-1_1;JavaAwt"/>
		<rdfs:subClassOf rdf:resource="&personaljava-1_1;JavaAwt"/>
		<rdfs:seeAlso rdf:resource="&j2se-1_2;JavaAwtEvent"/>
		<rdfs:seeAlso rdf:resource="&j2se-1_2;JavaText"/>
		<rdfs:seeAlso rdf:resource="&j2se-1_2;JavaAwtDnd"/>
		<rdfs:seeAlso rdf:resource="&j2se-1_2;JavaAwtDatatransfer"/>
		<rdfs:seeAlso rdf:resource="&j2se-1_2;JavaNet"/>
		<rdfs:seeAlso rdf:resource="&j2se-1_2;JavaAwtIm"/>
		<rdfs:seeAlso rdf:resource="&j2se-1_2;JavaAwtImageRenderable"/>
		<rdfs:seeAlso rdf:resource="&j2se-1_2;JavaLang"/>
		<rdfs:seeAlso rdf:resource="&j2se-1_2;JavaAwtFont"/>
		<rdfs:seeAlso rdf:resource="&j2se-1_2;JavaBeans"/>
		<rdfs:seeAlso rdf:resource="&j2se-1_2;JavaAwtColor"/>
		<rdfs:seeAlso rdf:resource="&j2se-1_2;JavaIo"/>
		<rdfs:seeAlso rdf:resource="&j2se-1_2;JavaUtil"/>
		<rdfs:seeAlso rdf:resource="&j2se-1_2;JavaSecurity"/>
		<rdfs:seeAlso rdf:resource="&j2se-1_2;JavaAwtImage"/>
		<rdfs:seeAlso rdf:resource="&j2se-1_2;JavaAwtGeom"/>
		<rdfs:comment xml:lang="en">Java API part implementing the java.awt package for J2SE 1.2</rdfs:comment>
	</owl:Class>
	<owl:Class rdf:about="&j2se-1_2;JavaAwtGeom">
		<rdfs:subClassOf rdf:resource="&java;JavaAPIPart"/>
		<rdfs:seeAlso rdf:resource="&j2se-1_2;JavaAwt"/>
		<rdfs:seeAlso rdf:resource="&j2se-1_2;JavaLang"/>
		<rdfs:seeAlso rdf:resource="&j2se-1_2;JavaIo"/>
		<rdfs:comment xml:lang="en">Java API part implementing the java.awt.geom package for J2SE 1.2</rdfs:comment>
	</owl:Class>
	<owl:Class rdf:about="&j2se-1_2;JavaAwtImage">
		<rdfs:subClassOf rdf:resource="&jdk-1_1;JavaAwtImage"/>
		<rdfs:subClassOf rdf:resource="&personaljava-1_1;JavaAwtImage"/>
		<rdfs:seeAlso rdf:resource="&j2se-1_2;JavaAwt"/>
		<rdfs:seeAlso rdf:resource="&j2se-1_2;JavaLang"/>
		<rdfs:seeAlso rdf:resource="&j2se-1_2;JavaAwtGeom"/>
		<rdfs:seeAlso rdf:resource="&j2se-1_2;JavaAwtColor"/>
		<rdfs:seeAlso rdf:resource="&j2se-1_2;JavaUtil"/>
		<rdfs:comment xml:lang="en">Java API part implementing the java.awt.image package for J2SE 1.2</rdfs:comment>
	</owl:Class>
	<owl:Class rdf:about="&j2se-1_2;JavaAwtImageRenderable">
		<rdfs:subClassOf rdf:resource="&java;JavaAPIPart"/>
		<rdfs:seeAlso rdf:resource="&j2se-1_2;JavaAwt"/>
		<rdfs:seeAlso rdf:resource="&j2se-1_2;JavaAwtImage"/>
		<rdfs:seeAlso rdf:resource="&j2se-1_2;JavaLang"/>
		<rdfs:seeAlso rdf:resource="&j2se-1_2;JavaAwtGeom"/>
		<rdfs:seeAlso rdf:resource="&j2se-1_2;JavaIo"/>
		<rdfs:seeAlso rdf:resource="&j2se-1_2;JavaUtil"/>
		<rdfs:comment xml:lang="en">Java API part implementing the java.awt.image.renderable package for J2SE 1.2</rdfs:comment>
	</owl:Class>
	<owl:Class rdf:about="&j2se-1_2;JavaAwtFont">
		<rdfs:subClassOf rdf:resource="&java;JavaAPIPart"/>
		<rdfs:seeAlso rdf:resource="&j2se-1_2;JavaAwt"/>
		<rdfs:seeAlso rdf:resource="&j2se-1_2;JavaLang"/>
		<rdfs:seeAlso rdf:resource="&j2se-1_2;JavaText"/>
		<rdfs:seeAlso rdf:resource="&j2se-1_2;JavaAwtGeom"/>
		<rdfs:seeAlso rdf:resource="&j2se-1_2;JavaIo"/>
		<rdfs:seeAlso rdf:resource="&j2se-1_2;JavaUtil"/>
		<rdfs:comment xml:lang="en">Java API part implementing the java.awt.font package for J2SE 1.2</rdfs:comment>
	</owl:Class>
	<owl:Class rdf:about="&j2se-1_2;JavaAwtEvent">
		<rdfs:subClassOf rdf:resource="&jdk-1_1;JavaAwtEvent"/>
		<rdfs:subClassOf rdf:resource="&personaljava-1_1;JavaAwtEvent"/>
		<rdfs:seeAlso rdf:resource="&j2se-1_2;JavaAwt"/>
		<rdfs:seeAlso rdf:resource="&j2se-1_2;JavaLang"/>
		<rdfs:seeAlso rdf:resource="&j2se-1_2;JavaText"/>
		<rdfs:seeAlso rdf:resource="&j2se-1_2;JavaAwtFont"/>
		<rdfs:seeAlso rdf:resource="&j2se-1_2;JavaUtil"/>
		<rdfs:comment xml:lang="en">Java API part implementing the java.awt.event package for J2SE 1.2</rdfs:comment>
	</owl:Class>
	<owl:Class rdf:about="&j2se-1_2;JavaAwtDnd">
		<rdfs:subClassOf rdf:resource="&java;JavaAPIPart"/>
		<rdfs:seeAlso rdf:resource="&j2se-1_2;JavaAwtEvent"/>
		<rdfs:seeAlso rdf:resource="&j2se-1_2;JavaAwtDatatransfer"/>
		<rdfs:seeAlso rdf:resource="&j2se-1_2;JavaIo"/>
		<rdfs:seeAlso rdf:resource="&j2se-1_2;JavaUtil"/>
		<rdfs:seeAlso rdf:resource="&j2se-1_2;JavaAwt"/>
		<rdfs:seeAlso rdf:resource="&j2se-1_2;JavaLang"/>
		<rdfs:comment xml:lang="en">Java API part implementing the java.awt.dnd package for J2SE 1.2</rdfs:comment>
	</owl:Class>
	<owl:Class rdf:about="&j2se-1_2;JavaAwtDatatransfer">
		<rdfs:subClassOf rdf:resource="&jdk-1_1;JavaAwtDatatransfer"/>
		<rdfs:subClassOf rdf:resource="&personaljava-1_1;JavaAwtDatatransfer"/>
		<rdfs:seeAlso rdf:resource="&j2se-1_2;JavaLang"/>
		<rdfs:seeAlso rdf:resource="&j2se-1_2;JavaIo"/>
		<rdfs:seeAlso rdf:resource="&j2se-1_2;JavaUtil"/>
		<rdfs:comment xml:lang="en">Java API part implementing the java.awt.datatransfer package for J2SE 1.2</rdfs:comment>
	</owl:Class>
	<owl:Class rdf:about="&j2se-1_2;JavaAwtIm">
		<rdfs:subClassOf rdf:resource="&java;JavaAPIPart"/>
		<rdfs:seeAlso rdf:resource="&j2se-1_2;JavaAwtFont"/>
		<rdfs:seeAlso rdf:resource="&j2se-1_2;JavaAwt"/>
		<rdfs:seeAlso rdf:resource="&j2se-1_2;JavaLang"/>
		<rdfs:seeAlso rdf:resource="&j2se-1_2;JavaText"/>
		<rdfs:seeAlso rdf:resource="&j2se-1_2;JavaUtil"/>
		<rdfs:comment xml:lang="en">Java API part implementing the java.awt.im package for J2SE 1.2</rdfs:comment>
	</owl:Class>
	<owl:Class rdf:about="&j2se-1_2;JavaAwtPrint">
		<rdfs:subClassOf rdf:resource="&java;JavaAPIPart"/>
		<rdfs:seeAlso rdf:resource="&j2se-1_2;JavaAwt"/>
		<rdfs:seeAlso rdf:resource="&j2se-1_2;JavaLang"/>
		<rdfs:seeAlso rdf:resource="&j2se-1_2;JavaIo"/>
		<rdfs:comment xml:lang="en">Java API part implementing the java.awt.print package for J2SE 1.2</rdfs:comment>
	</owl:Class>
	<owl:Class rdf:about="&j2se-1_2;JavaAwtColor">
		<rdfs:subClassOf rdf:resource="&java;JavaAPIPart"/>
		<rdfs:seeAlso rdf:resource="&j2se-1_2;JavaLang"/>
		<rdfs:seeAlso rdf:resource="&j2se-1_2;JavaIo"/>
		<rdfs:comment xml:lang="en">Java API part implementing the java.awt.color package for J2SE 1.2</rdfs:comment>
	</owl:Class>
	<owl:Class rdf:about="&j2se-1_2;JavaBeans">
		<rdfs:subClassOf rdf:resource="&jdk-1_1;JavaBeans"/>
		<rdfs:subClassOf rdf:resource="&personaljava-1_1;JavaBeans"/>
		<rdfs:seeAlso rdf:resource="&j2se-1_2;JavaAwt"/>
		<rdfs:seeAlso rdf:resource="&j2se-1_2;JavaApplet"/>
		<rdfs:seeAlso rdf:resource="&j2se-1_2;JavaLang"/>
		<rdfs:seeAlso rdf:resource="&j2se-1_2;JavaBeansBeancontext"/>
		<rdfs:seeAlso rdf:resource="&j2se-1_2;JavaLangReflect"/>
		<rdfs:seeAlso rdf:resource="&j2se-1_2;JavaIo"/>
		<rdfs:seeAlso rdf:resource="&j2se-1_2;JavaUtil"/>
		<rdfs:comment xml:lang="en">Java API part implementing the java.beans package for J2SE 1.2</rdfs:comment>
	</owl:Class>
	<owl:Class rdf:about="&j2se-1_2;JavaBeansBeancontext">
		<rdfs:subClassOf rdf:resource="&java;JavaAPIPart"/>
		<rdfs:seeAlso rdf:resource="&j2se-1_2;JavaNet"/>
		<rdfs:seeAlso rdf:resource="&j2se-1_2;JavaIo"/>
		<rdfs:seeAlso rdf:resource="&j2se-1_2;JavaUtil"/>
		<rdfs:seeAlso rdf:resource="&j2se-1_2;JavaAwt"/>
		<rdfs:seeAlso rdf:resource="&j2se-1_2;JavaLang"/>
		<rdfs:seeAlso rdf:resource="&j2se-1_2;JavaBeans"/>
		<rdfs:comment xml:lang="en">Java API part implementing the java.beans.beancontext package for J2SE 1.2</rdfs:comment>
	</owl:Class>
	<owl:Class rdf:about="&j2se-1_2;JavaApplet">
		<rdfs:subClassOf rdf:resource="&jdk-1_1;JavaApplet"/>
		<rdfs:subClassOf rdf:resource="&personaljava-1_1;JavaApplet"/>
		<rdfs:seeAlso rdf:resource="&j2se-1_2;JavaAwt"/>
		<rdfs:seeAlso rdf:resource="&j2se-1_2;JavaLang"/>
		<rdfs:seeAlso rdf:resource="&j2se-1_2;JavaNet"/>
		<rdfs:seeAlso rdf:resource="&j2se-1_2;JavaUtil"/>
		<rdfs:comment xml:lang="en">Java API part implementing the java.applet package for J2SE 1.2</rdfs:comment>
	</owl:Class>
	<owl:Class rdf:about="&j2se-1_2;JavaRmi">
		<rdfs:subClassOf rdf:resource="&jdk-1_1;JavaRmi"/>
		<rdfs:seeAlso rdf:resource="&j2se-1_2;JavaLang"/>
		<rdfs:seeAlso rdf:resource="&j2se-1_2;JavaIo"/>
		<rdfs:comment xml:lang="en">Java API part implementing the java.rmi package for J2SE 1.2</rdfs:comment>
	</owl:Class>
	<owl:Class rdf:about="&j2se-1_2;JavaRmiServer">
		<rdfs:subClassOf rdf:resource="&jdk-1_1;JavaRmiServer"/>
		<rdfs:seeAlso rdf:resource="&j2se-1_2;JavaRmi"/>
		<rdfs:seeAlso rdf:resource="&j2se-1_2;JavaLang"/>
		<rdfs:seeAlso rdf:resource="&j2se-1_2;JavaLangReflect"/>
		<rdfs:seeAlso rdf:resource="&j2se-1_2;JavaNet"/>
		<rdfs:seeAlso rdf:resource="&j2se-1_2;JavaIo"/>
		<rdfs:comment xml:lang="en">Java API part implementing the java.rmi.server package for J2SE 1.2</rdfs:comment>
	</owl:Class>
	<owl:Class rdf:about="&j2se-1_2;JavaRmiDgc">
		<owl:equivalentClass rdf:resource="&jdk-1_1;JavaRmiDgc"/>
		<rdfs:subClassOf rdf:resource="&java;JavaAPIPart"/>
		<rdfs:seeAlso rdf:resource="&j2se-1_2;JavaRmi"/>
		<rdfs:seeAlso rdf:resource="&j2se-1_2;JavaLang"/>
		<rdfs:seeAlso rdf:resource="&j2se-1_2;JavaIo"/>
		<rdfs:comment xml:lang="en">Java API part implementing the java.rmi.dgc package for J2SE 1.2</rdfs:comment>
	</owl:Class>
	<owl:Class rdf:about="&j2se-1_2;JavaRmiRegistry">
		<rdfs:subClassOf rdf:resource="&jdk-1_1;JavaRmiRegistry"/>
		<rdfs:seeAlso rdf:resource="&j2se-1_2;JavaRmi"/>
		<rdfs:seeAlso rdf:resource="&j2se-1_2;JavaLang"/>
		<rdfs:seeAlso rdf:resource="&j2se-1_2;JavaRmiServer"/>
		<rdfs:comment xml:lang="en">Java API part implementing the java.rmi.registry package for J2SE 1.2</rdfs:comment>
	</owl:Class>
	<owl:Class rdf:about="&j2se-1_2;JavaRmiActivation">
		<rdfs:subClassOf rdf:resource="&java;JavaAPIPart"/>
		<rdfs:seeAlso rdf:resource="&j2se-1_2;JavaRmi"/>
		<rdfs:seeAlso rdf:resource="&j2se-1_2;JavaLang"/>
		<rdfs:seeAlso rdf:resource="&j2se-1_2;JavaRmiServer"/>
		<rdfs:seeAlso rdf:resource="&j2se-1_2;JavaIo"/>
		<rdfs:seeAlso rdf:resource="&j2se-1_2;JavaUtil"/>
		<rdfs:comment xml:lang="en">Java API part implementing the java.rmi.activation package for J2SE 1.2</rdfs:comment>
	</owl:Class>
	<owl:Class rdf:about="&j2se-1_2;JavaSql">
		<rdfs:subClassOf rdf:resource="&jdk-1_1;JavaSql"/>
		<rdfs:seeAlso rdf:resource="&j2se-1_2;JavaLang"/>
		<rdfs:seeAlso rdf:resource="&j2se-1_2;JavaMath"/>
		<rdfs:seeAlso rdf:resource="&j2se-1_2;JavaIo"/>
		<rdfs:seeAlso rdf:resource="&j2se-1_2;JavaUtil"/>
		<rdfs:comment xml:lang="en">Java API part implementing the java.sql package for J2SE 1.2</rdfs:comment>
	</owl:Class>
	<owl:Class rdf:about="&j2se-1_2;JavaxSwing">
		<rdfs:subClassOf rdf:resource="&java;JavaAPIPart"/>
		<rdfs:seeAlso rdf:resource="&j2se-1_2;JavaAwtEvent"/>
		<rdfs:seeAlso rdf:resource="&j2se-1_2;JavaText"/>
		<rdfs:seeAlso rdf:resource="&j2se-1_2;JavaxSwingEvent"/>
		<rdfs:seeAlso rdf:resource="&j2se-1_2;JavaxSwingColorchooser"/>
		<rdfs:seeAlso rdf:resource="&j2se-1_2;JavaNet"/>
		<rdfs:seeAlso rdf:resource="&j2se-1_2;JavaxSwingTable"/>
		<rdfs:seeAlso rdf:resource="&j2se-1_2;JavaAwt"/>
		<rdfs:seeAlso rdf:resource="&j2se-1_2;JavaxAccessibility"/>
		<rdfs:seeAlso rdf:resource="&j2se-1_2;JavaBeans"/>
		<rdfs:seeAlso rdf:resource="&j2se-1_2;JavaxSwingPlaf"/>
		<rdfs:seeAlso rdf:resource="&j2se-1_2;JavaApplet"/>
		<rdfs:seeAlso rdf:resource="&j2se-1_2;JavaxSwingBorder"/>
		<rdfs:seeAlso rdf:resource="&j2se-1_2;JavaIo"/>
		<rdfs:seeAlso rdf:resource="&j2se-1_2;JavaUtil"/>
		<rdfs:seeAlso rdf:resource="&j2se-1_2;JavaAwtImage"/>
		<rdfs:seeAlso rdf:resource="&j2se-1_2;JavaxSwingText"/>
		<rdfs:seeAlso rdf:resource="&j2se-1_2;JavaLang"/>
		<rdfs:seeAlso rdf:resource="&j2se-1_2;JavaxSwingTree"/>
		<rdfs:seeAlso rdf:resource="&j2se-1_2;JavaxSwingFilechooser"/>
		<rdfs:comment xml:lang="en">Java API part implementing the javax.swing package for J2SE 1.2</rdfs:comment>
	</owl:Class>
	<owl:Class rdf:about="&j2se-1_2;JavaxSwingEvent">
		<rdfs:subClassOf rdf:resource="&java;JavaAPIPart"/>
		<rdfs:seeAlso rdf:resource="&j2se-1_2;JavaAwtEvent"/>
		<rdfs:seeAlso rdf:resource="&j2se-1_2;JavaxSwingUndo"/>
		<rdfs:seeAlso rdf:resource="&j2se-1_2;JavaNet"/>
		<rdfs:seeAlso rdf:resource="&j2se-1_2;JavaIo"/>
		<rdfs:seeAlso rdf:resource="&j2se-1_2;JavaUtil"/>
		<rdfs:seeAlso rdf:resource="&j2se-1_2;JavaAwt"/>
		<rdfs:seeAlso rdf:resource="&j2se-1_2;JavaxSwingTable"/>
		<rdfs:seeAlso rdf:resource="&j2se-1_2;JavaxSwing"/>
		<rdfs:seeAlso rdf:resource="&j2se-1_2;JavaLang"/>
		<rdfs:seeAlso rdf:resource="&j2se-1_2;JavaxSwingTree"/>
		<rdfs:seeAlso rdf:resource="&j2se-1_2;JavaBeans"/>
		<rdfs:seeAlso rdf:resource="&j2se-1_2;JavaxSwingText"/>
		<rdfs:comment xml:lang="en">Java API part implementing the javax.swing.event package for J2SE 1.2</rdfs:comment>
	</owl:Class>
	<owl:Class rdf:about="&j2se-1_2;JavaxSwingText">
		<rdfs:subClassOf rdf:resource="&java;JavaAPIPart"/>
		<rdfs:seeAlso rdf:resource="&j2se-1_2;JavaAwtEvent"/>
		<rdfs:seeAlso rdf:resource="&j2se-1_2;JavaxSwingEvent"/>
		<rdfs:seeAlso rdf:resource="&j2se-1_2;JavaxSwingUndo"/>
		<rdfs:seeAlso rdf:resource="&j2se-1_2;JavaAwtIm"/>
		<rdfs:seeAlso rdf:resource="&j2se-1_2;JavaAwt"/>
		<rdfs:seeAlso rdf:resource="&j2se-1_2;JavaxAccessibility"/>
		<rdfs:seeAlso rdf:resource="&j2se-1_2;JavaLang"/>
		<rdfs:seeAlso rdf:resource="&j2se-1_2;JavaxSwingTree"/>
		<rdfs:seeAlso rdf:resource="&j2se-1_2;JavaxSwingPlaf"/>
		<rdfs:seeAlso rdf:resource="&j2se-1_2;JavaxSwingPlafBasic"/>
		<rdfs:seeAlso rdf:resource="&j2se-1_2;JavaIo"/>
		<rdfs:seeAlso rdf:resource="&j2se-1_2;JavaUtil"/>
		<rdfs:seeAlso rdf:resource="&j2se-1_2;JavaxSwing"/>
		<rdfs:comment xml:lang="en">Java API part implementing the javax.swing.text package for J2SE 1.2</rdfs:comment>
	</owl:Class>
	<owl:Class rdf:about="&j2se-1_2;JavaxSwingTextHtml">
		<rdfs:subClassOf rdf:resource="&java;JavaAPIPart"/>
		<rdfs:seeAlso rdf:resource="&j2se-1_2;JavaAwtEvent"/>
		<rdfs:seeAlso rdf:resource="&j2se-1_2;JavaxSwingEvent"/>
		<rdfs:seeAlso rdf:resource="&j2se-1_2;JavaNet"/>
		<rdfs:seeAlso rdf:resource="&j2se-1_2;JavaIo"/>
		<rdfs:seeAlso rdf:resource="&j2se-1_2;JavaUtil"/>
		<rdfs:seeAlso rdf:resource="&j2se-1_2;JavaAwt"/>
		<rdfs:seeAlso rdf:resource="&j2se-1_2;JavaxSwing"/>
		<rdfs:seeAlso rdf:resource="&j2se-1_2;JavaLang"/>
		<rdfs:seeAlso rdf:resource="&j2se-1_2;JavaxSwingText"/>
		<rdfs:comment xml:lang="en">Java API part implementing the javax.swing.text.html package for J2SE 1.2</rdfs:comment>
	</owl:Class>
	<owl:Class rdf:about="&j2se-1_2;JavaxSwingTextHtmlParser">
		<rdfs:subClassOf rdf:resource="&java;JavaAPIPart"/>
		<rdfs:seeAlso rdf:resource="&j2se-1_2;JavaxSwingTextHtml"/>
		<rdfs:seeAlso rdf:resource="&j2se-1_2;JavaLang"/>
		<rdfs:seeAlso rdf:resource="&j2se-1_2;JavaIo"/>
		<rdfs:seeAlso rdf:resource="&j2se-1_2;JavaxSwingText"/>
		<rdfs:seeAlso rdf:resource="&j2se-1_2;JavaUtil"/>
		<rdfs:comment xml:lang="en">Java API part implementing the javax.swing.text.html.parser package for J2SE 1.2</rdfs:comment>
	</owl:Class>
	<owl:Class rdf:about="&j2se-1_2;JavaxSwingTextRtf">
		<rdfs:subClassOf rdf:resource="&java;JavaAPIPart"/>
		<rdfs:seeAlso rdf:resource="&j2se-1_2;JavaLang"/>
		<rdfs:seeAlso rdf:resource="&j2se-1_2;JavaxSwingText"/>
		<rdfs:seeAlso rdf:resource="&j2se-1_2;JavaIo"/>
		<rdfs:comment xml:lang="en">Java API part implementing the javax.swing.text.rtf package for J2SE 1.2</rdfs:comment>
	</owl:Class>
	<owl:Class rdf:about="&j2se-1_2;JavaxSwingUndo">
		<rdfs:subClassOf rdf:resource="&java;JavaAPIPart"/>
		<rdfs:seeAlso rdf:resource="&j2se-1_2;JavaLang"/>
		<rdfs:seeAlso rdf:resource="&j2se-1_2;JavaxSwingEvent"/>
		<rdfs:seeAlso rdf:resource="&j2se-1_2;JavaIo"/>
		<rdfs:seeAlso rdf:resource="&j2se-1_2;JavaUtil"/>
		<rdfs:comment xml:lang="en">Java API part implementing the javax.swing.undo package for J2SE 1.2</rdfs:comment>
	</owl:Class>
	<owl:Class rdf:about="&j2se-1_2;JavaxSwingTable">
		<rdfs:subClassOf rdf:resource="&java;JavaAPIPart"/>
		<rdfs:seeAlso rdf:resource="&j2se-1_2;JavaxSwingPlaf"/>
		<rdfs:seeAlso rdf:resource="&j2se-1_2;JavaAwtEvent"/>
		<rdfs:seeAlso rdf:resource="&j2se-1_2;JavaxSwingEvent"/>
		<rdfs:seeAlso rdf:resource="&j2se-1_2;JavaxSwingBorder"/>
		<rdfs:seeAlso rdf:resource="&j2se-1_2;JavaIo"/>
		<rdfs:seeAlso rdf:resource="&j2se-1_2;JavaUtil"/>
		<rdfs:seeAlso rdf:resource="&j2se-1_2;JavaAwt"/>
		<rdfs:seeAlso rdf:resource="&j2se-1_2;JavaxSwing"/>
		<rdfs:seeAlso rdf:resource="&j2se-1_2;JavaxAccessibility"/>
		<rdfs:seeAlso rdf:resource="&j2se-1_2;JavaLang"/>
		<rdfs:seeAlso rdf:resource="&j2se-1_2;JavaBeans"/>
		<rdfs:comment xml:lang="en">Java API part implementing the javax.swing.table package for J2SE 1.2</rdfs:comment>
	</owl:Class>
	<owl:Class rdf:about="&j2se-1_2;JavaxSwingTree">
		<rdfs:subClassOf rdf:resource="&java;JavaAPIPart"/>
		<rdfs:seeAlso rdf:resource="&j2se-1_2;JavaAwtEvent"/>
		<rdfs:seeAlso rdf:resource="&j2se-1_2;JavaxSwingEvent"/>
		<rdfs:seeAlso rdf:resource="&j2se-1_2;JavaxSwingBorder"/>
		<rdfs:seeAlso rdf:resource="&j2se-1_2;JavaIo"/>
		<rdfs:seeAlso rdf:resource="&j2se-1_2;JavaUtil"/>
		<rdfs:seeAlso rdf:resource="&j2se-1_2;JavaAwt"/>
		<rdfs:seeAlso rdf:resource="&j2se-1_2;JavaxSwing"/>
		<rdfs:seeAlso rdf:resource="&j2se-1_2;JavaLang"/>
		<rdfs:seeAlso rdf:resource="&j2se-1_2;JavaBeans"/>
		<rdfs:comment xml:lang="en">Java API part implementing the javax.swing.tree package for J2SE 1.2</rdfs:comment>
	</owl:Class>
	<owl:Class rdf:about="&j2se-1_2;JavaxSwingPlaf">
		<rdfs:subClassOf rdf:resource="&java;JavaAPIPart"/>
		<rdfs:seeAlso rdf:resource="&j2se-1_2;JavaxSwingBorder"/>
		<rdfs:seeAlso rdf:resource="&j2se-1_2;JavaIo"/>
		<rdfs:seeAlso rdf:resource="&j2se-1_2;JavaAwt"/>
		<rdfs:seeAlso rdf:resource="&j2se-1_2;JavaxSwing"/>
		<rdfs:seeAlso rdf:resource="&j2se-1_2;JavaxAccessibility"/>
		<rdfs:seeAlso rdf:resource="&j2se-1_2;JavaLang"/>
		<rdfs:seeAlso rdf:resource="&j2se-1_2;JavaxSwingFilechooser"/>
		<rdfs:seeAlso rdf:resource="&j2se-1_2;JavaxSwingTree"/>
		<rdfs:seeAlso rdf:resource="&j2se-1_2;JavaxSwingText"/>
		<rdfs:comment xml:lang="en">Java API part implementing the javax.swing.plaf package for J2SE 1.2</rdfs:comment>
	</owl:Class>
	<owl:Class rdf:about="&j2se-1_2;JavaxSwingPlafBasic">
		<rdfs:subClassOf rdf:resource="&java;JavaAPIPart"/>
		<rdfs:seeAlso rdf:resource="&j2se-1_2;JavaAwtEvent"/>
		<rdfs:seeAlso rdf:resource="&j2se-1_2;JavaxSwingEvent"/>
		<rdfs:seeAlso rdf:resource="&j2se-1_2;JavaxSwingTable"/>
		<rdfs:seeAlso rdf:resource="&j2se-1_2;JavaAwt"/>
		<rdfs:seeAlso rdf:resource="&j2se-1_2;JavaxAccessibility"/>
		<rdfs:seeAlso rdf:resource="&j2se-1_2;JavaBeans"/>
		<rdfs:seeAlso rdf:resource="&j2se-1_2;JavaxSwingPlaf"/>
		<rdfs:seeAlso rdf:resource="&j2se-1_2;JavaxSwingBorder"/>
		<rdfs:seeAlso rdf:resource="&j2se-1_2;JavaIo"/>
		<rdfs:seeAlso rdf:resource="&j2se-1_2;JavaUtil"/>
		<rdfs:seeAlso rdf:resource="&j2se-1_2;JavaxSwing"/>
		<rdfs:seeAlso rdf:resource="&j2se-1_2;JavaxSwingText"/>
		<rdfs:seeAlso rdf:resource="&j2se-1_2;JavaLang"/>
		<rdfs:seeAlso rdf:resource="&j2se-1_2;JavaxSwingTree"/>
		<rdfs:seeAlso rdf:resource="&j2se-1_2;JavaxSwingFilechooser"/>
		<rdfs:comment xml:lang="en">Java API part implementing the javax.swing.plaf.basic package for J2SE 1.2</rdfs:comment>
	</owl:Class>
	<owl:Class rdf:about="&j2se-1_2;JavaxSwingPlafMetal">
		<rdfs:subClassOf rdf:resource="&java;JavaAPIPart"/>
		<rdfs:seeAlso rdf:resource="&j2se-1_2;JavaAwtEvent"/>
		<rdfs:seeAlso rdf:resource="&j2se-1_2;JavaxSwingEvent"/>
		<rdfs:seeAlso rdf:resource="&j2se-1_2;JavaAwt"/>
		<rdfs:seeAlso rdf:resource="&j2se-1_2;JavaLang"/>
		<rdfs:seeAlso rdf:resource="&j2se-1_2;JavaxSwingTree"/>
		<rdfs:seeAlso rdf:resource="&j2se-1_2;JavaBeans"/>
		<rdfs:seeAlso rdf:resource="&j2se-1_2;JavaxSwingPlaf"/>
		<rdfs:seeAlso rdf:resource="&j2se-1_2;JavaxSwingPlafBasic"/>
		<rdfs:seeAlso rdf:resource="&j2se-1_2;JavaxSwingBorder"/>
		<rdfs:seeAlso rdf:resource="&j2se-1_2;JavaIo"/>
		<rdfs:seeAlso rdf:resource="&j2se-1_2;JavaxSwing"/>
		<rdfs:comment xml:lang="en">Java API part implementing the javax.swing.plaf.metal package for J2SE 1.2</rdfs:comment>
	</owl:Class>
	<owl:Class rdf:about="&j2se-1_2;JavaxSwingPlafMulti">
		<rdfs:subClassOf rdf:resource="&java;JavaAPIPart"/>
		<rdfs:seeAlso rdf:resource="&j2se-1_2;JavaAwt"/>
		<rdfs:seeAlso rdf:resource="&j2se-1_2;JavaxAccessibility"/>
		<rdfs:seeAlso rdf:resource="&j2se-1_2;JavaLang"/>
		<rdfs:seeAlso rdf:resource="&j2se-1_2;JavaxSwingTree"/>
		<rdfs:seeAlso rdf:resource="&j2se-1_2;JavaxSwingPlaf"/>
		<rdfs:seeAlso rdf:resource="&j2se-1_2;JavaIo"/>
		<rdfs:seeAlso rdf:resource="&j2se-1_2;JavaUtil"/>
		<rdfs:seeAlso rdf:resource="&j2se-1_2;JavaxSwing"/>
		<rdfs:seeAlso rdf:resource="&j2se-1_2;JavaxSwingFilechooser"/>
		<rdfs:seeAlso rdf:resource="&j2se-1_2;JavaxSwingText"/>
		<rdfs:comment xml:lang="en">Java API part implementing the javax.swing.plaf.multi package for J2SE 1.2</rdfs:comment>
	</owl:Class>
	<owl:Class rdf:about="&j2se-1_2;JavaxSwingBorder">
		<rdfs:subClassOf rdf:resource="&java;JavaAPIPart"/>
		<rdfs:seeAlso rdf:resource="&j2se-1_2;JavaAwt"/>
		<rdfs:seeAlso rdf:resource="&j2se-1_2;JavaxSwing"/>
		<rdfs:seeAlso rdf:resource="&j2se-1_2;JavaLang"/>
		<rdfs:seeAlso rdf:resource="&j2se-1_2;JavaIo"/>
		<rdfs:comment xml:lang="en">Java API part implementing the javax.swing.border package for J2SE 1.2</rdfs:comment>
	</owl:Class>
	<owl:Class rdf:about="&j2se-1_2;JavaxSwingColorchooser">
		<rdfs:subClassOf rdf:resource="&java;JavaAPIPart"/>
		<rdfs:seeAlso rdf:resource="&j2se-1_2;JavaAwt"/>
		<rdfs:seeAlso rdf:resource="&j2se-1_2;JavaxSwing"/>
		<rdfs:seeAlso rdf:resource="&j2se-1_2;JavaLang"/>
		<rdfs:seeAlso rdf:resource="&j2se-1_2;JavaxSwingEvent"/>
		<rdfs:seeAlso rdf:resource="&j2se-1_2;JavaIo"/>
		<rdfs:comment xml:lang="en">Java API part implementing the javax.swing.colorchooser package for J2SE 1.2</rdfs:comment>
	</owl:Class>
	<owl:Class rdf:about="&j2se-1_2;JavaxSwingFilechooser">
		<rdfs:subClassOf rdf:resource="&java;JavaAPIPart"/>
		<rdfs:seeAlso rdf:resource="&j2se-1_2;JavaxSwing"/>
		<rdfs:seeAlso rdf:resource="&j2se-1_2;JavaLang"/>
		<rdfs:seeAlso rdf:resource="&j2se-1_2;JavaIo"/>
		<rdfs:comment xml:lang="en">Java API part implementing the javax.swing.filechooser package for J2SE 1.2</rdfs:comment>
	</owl:Class>
	<owl:Class rdf:about="&j2se-1_2;JavaxAccessibility">
		<rdfs:subClassOf rdf:resource="&java;JavaAPIPart"/>
		<rdfs:seeAlso rdf:resource="&j2se-1_2;JavaAwtEvent"/>
		<rdfs:seeAlso rdf:resource="&j2se-1_2;JavaAwt"/>
		<rdfs:seeAlso rdf:resource="&j2se-1_2;JavaLang"/>
		<rdfs:seeAlso rdf:resource="&j2se-1_2;JavaBeans"/>
		<rdfs:seeAlso rdf:resource="&j2se-1_2;JavaxSwingText"/>
		<rdfs:seeAlso rdf:resource="&j2se-1_2;JavaUtil"/>
		<rdfs:comment xml:lang="en">Java API part implementing the javax.accessibility package for J2SE 1.2</rdfs:comment>
	</owl:Class>
	<owl:Class rdf:about="&j2se-1_2;OrgOmgCORBA">
		<rdfs:subClassOf rdf:resource="&java;JavaAPIPart"/>
		<rdfs:seeAlso rdf:resource="&j2se-1_2;JavaApplet"/>
		<rdfs:seeAlso rdf:resource="&j2se-1_2;JavaLang"/>
		<rdfs:seeAlso rdf:resource="&j2se-1_2;JavaMath"/>
		<rdfs:seeAlso rdf:resource="&j2se-1_2;OrgOmgCORBAPortable"/>
		<rdfs:seeAlso rdf:resource="&j2se-1_2;JavaIo"/>
		<rdfs:seeAlso rdf:resource="&j2se-1_2;JavaUtil"/>
		<rdfs:comment xml:lang="en">Java API part implementing the org.omg.CORBA package for J2SE 1.2</rdfs:comment>
	</owl:Class>
	<owl:Class rdf:about="&j2se-1_2;OrgOmgCORBAPortable">
		<rdfs:subClassOf rdf:resource="&java;JavaAPIPart"/>
		<rdfs:seeAlso rdf:resource="&j2se-1_2;JavaLang"/>
		<rdfs:seeAlso rdf:resource="&j2se-1_2;JavaMath"/>
		<rdfs:seeAlso rdf:resource="&j2se-1_2;JavaIo"/>
		<rdfs:seeAlso rdf:resource="&j2se-1_2;OrgOmgCORBA"/>
		<rdfs:comment xml:lang="en">Java API part implementing the org.omg.CORBA.portable package for J2SE 1.2</rdfs:comment>
	</owl:Class>
	<owl:Class rdf:about="&j2se-1_2;OrgOmgCORBADynAnyPackage">
		<rdfs:subClassOf rdf:resource="&java;JavaAPIPart"/>
		<rdfs:seeAlso rdf:resource="&j2se-1_2;JavaLang"/>
		<rdfs:seeAlso rdf:resource="&j2se-1_2;OrgOmgCORBA"/>
		<rdfs:comment xml:lang="en">Java API part implementing the org.omg.CORBA.DynAnyPackage package for J2SE 1.2</rdfs:comment>
	</owl:Class>
	<owl:Class rdf:about="&j2se-1_2;OrgOmgCORBAORBPackage">
		<rdfs:subClassOf rdf:resource="&java;JavaAPIPart"/>
		<rdfs:seeAlso rdf:resource="&j2se-1_2;JavaLang"/>
		<rdfs:seeAlso rdf:resource="&j2se-1_2;OrgOmgCORBA"/>
		<rdfs:comment xml:lang="en">Java API part implementing the org.omg.CORBA.ORBPackage package for J2SE 1.2</rdfs:comment>
	</owl:Class>
	<owl:Class rdf:about="&j2se-1_2;OrgOmgCORBATypeCodePackage">
		<rdfs:subClassOf rdf:resource="&java;JavaAPIPart"/>
		<rdfs:seeAlso rdf:resource="&j2se-1_2;JavaLang"/>
		<rdfs:seeAlso rdf:resource="&j2se-1_2;OrgOmgCORBA"/>
		<rdfs:comment xml:lang="en">Java API part implementing the org.omg.CORBA.TypeCodePackage package for J2SE 1.2</rdfs:comment>
	</owl:Class>
	<owl:Class rdf:about="&j2se-1_2;OrgOmgCosNaming">
		<rdfs:subClassOf rdf:resource="&java;JavaAPIPart"/>
		<rdfs:seeAlso rdf:resource="&j2se-1_2;JavaLang"/>
		<rdfs:seeAlso rdf:resource="&j2se-1_2;OrgOmgCORBAPortable"/>
		<rdfs:seeAlso rdf:resource="&j2se-1_2;OrgOmgCORBA"/>
		<rdfs:comment xml:lang="en">Java API part implementing the org.omg.CosNaming package for J2SE 1.2</rdfs:comment>
	</owl:Class>
	<owl:Class rdf:about="&j2se-1_2;OrgOmgCosNamingNamingContextPackage">
		<rdfs:subClassOf rdf:resource="&java;JavaAPIPart"/>
		<rdfs:seeAlso rdf:resource="&j2se-1_2;OrgOmgCosNaming"/>
		<rdfs:seeAlso rdf:resource="&j2se-1_2;JavaLang"/>
		<rdfs:seeAlso rdf:resource="&j2se-1_2;OrgOmgCORBAPortable"/>
		<rdfs:seeAlso rdf:resource="&j2se-1_2;OrgOmgCORBA"/>
		<rdfs:comment xml:lang="en">Java API part implementing the org.omg.CosNaming.NamingContextPackage package for J2SE 1.2</rdfs:comment>
	</owl:Class>
	<owl:Class rdf:about="&j2se-1_2;JavaIoAPI">
		<rdfs:subClassOf rdf:resource="&jdk-1_1;JavaIoAPI"/>
		<rdfs:subClassOf rdf:resource="&j2me-midp-2_0;JavaIoAPI"/>
		<rdfs:subClassOf rdf:resource="&personaljava-1_1;JavaIoAPI"/>
		<rdfs:comment xml:lang="en">JavaLibrary implementing the java.io package for J2SE 1.2</rdfs:comment>
		<rdfs:comment xml:lang="OWLManchester">platform:comprisesInterfacePart some JavaIo</rdfs:comment>
	</owl:Class>
	<owl:Class rdf:about="&j2se-1_2;JavaLangAPI">
		<rdfs:subClassOf rdf:resource="&j2me-midp-2_0;JavaLangAPI"/>
		<rdfs:comment xml:lang="en">JavaLibrary implementing the java.lang package for J2SE 1.2</rdfs:comment>
		<rdfs:comment xml:lang="OWLManchester">platform:comprisesInterfacePart some JavaLang</rdfs:comment>
	</owl:Class>
	<owl:Class rdf:about="&j2se-1_2;JavaLangReflectAPI">
		<rdfs:subClassOf rdf:resource="&jdk-1_1;JavaLangReflectAPI"/>
		<rdfs:subClassOf rdf:resource="&personaljava-1_1;JavaLangReflectAPI"/>
		<rdfs:comment xml:lang="en">JavaLibrary implementing the java.lang.reflect package for J2SE 1.2</rdfs:comment>
		<rdfs:comment xml:lang="OWLManchester">platform:comprisesInterfacePart some JavaLangReflect</rdfs:comment>
	</owl:Class>
	<owl:Class rdf:about="&j2se-1_2;JavaLangRefAPI">
		<rdfs:subClassOf rdf:resource="&java;JavaAPI"/>
		<rdfs:comment xml:lang="en">JavaLibrary implementing the java.lang.ref package for J2SE 1.2</rdfs:comment>
		<rdfs:comment xml:lang="OWLManchester">platform:comprisesInterfacePart some JavaLangRef</rdfs:comment>
	</owl:Class>
	<owl:Class rdf:about="&j2se-1_2;JavaNetAPI">
		<rdfs:subClassOf rdf:resource="&jdk-1_1;JavaNetAPI"/>
		<rdfs:subClassOf rdf:resource="&personaljava-1_1;JavaNetAPI"/>
		<rdfs:comment xml:lang="en">JavaLibrary implementing the java.net package for J2SE 1.2</rdfs:comment>
		<rdfs:comment xml:lang="OWLManchester">platform:comprisesInterfacePart some JavaNet</rdfs:comment>
	</owl:Class>
	<owl:Class rdf:about="&j2se-1_2;JavaSecurityAPI">
		<rdfs:subClassOf rdf:resource="&jdk-1_1;JavaSecurityAPI"/>
		<rdfs:comment xml:lang="en">JavaLibrary implementing the java.security package for J2SE 1.2</rdfs:comment>
		<rdfs:comment xml:lang="OWLManchester">platform:comprisesInterfacePart some JavaSecurity</rdfs:comment>
	</owl:Class>
	<owl:Class rdf:about="&j2se-1_2;JavaSecurityCertAPI">
		<rdfs:subClassOf rdf:resource="&java;JavaAPI"/>
		<rdfs:comment xml:lang="en">JavaLibrary implementing the java.security.cert package for J2SE 1.2</rdfs:comment>
		<rdfs:comment xml:lang="OWLManchester">platform:comprisesInterfacePart some JavaSecurityCert</rdfs:comment>
	</owl:Class>
	<owl:Class rdf:about="&j2se-1_2;JavaSecuritySpecAPI">
		<rdfs:subClassOf rdf:resource="&java;JavaAPI"/>
		<rdfs:comment xml:lang="en">JavaLibrary implementing the java.security.spec package for J2SE 1.2</rdfs:comment>
		<rdfs:comment xml:lang="OWLManchester">platform:comprisesInterfacePart some JavaSecuritySpec</rdfs:comment>
	</owl:Class>
	<owl:Class rdf:about="&j2se-1_2;JavaSecurityInterfacesAPI">
		<rdfs:subClassOf rdf:resource="&jdk-1_1;JavaSecurityInterfacesAPI"/>
		<rdfs:comment xml:lang="en">JavaLibrary implementing the java.security.interfaces package for J2SE 1.2</rdfs:comment>
		<rdfs:comment xml:lang="OWLManchester">platform:comprisesInterfacePart some JavaSecurityInterfaces</rdfs:comment>
	</owl:Class>
	<owl:Class rdf:about="&j2se-1_2;JavaSecurityAclAPI">
		<owl:equivalentClass rdf:resource="&jdk-1_1;JavaSecurityAclAPI"/>
		<rdfs:subClassOf rdf:resource="&java;JavaAPI"/>
		<rdfs:comment xml:lang="en">JavaLibrary implementing the java.security.acl package for J2SE 1.2</rdfs:comment>
		<rdfs:comment xml:lang="OWLManchester">platform:comprisesInterfacePart some JavaSecurityAcl</rdfs:comment>
	</owl:Class>
	<owl:Class rdf:about="&j2se-1_2;JavaUtilAPI">
		<rdfs:subClassOf rdf:resource="&jdk-1_1;JavaUtilAPI"/>
		<rdfs:subClassOf rdf:resource="&personaljava-1_1;JavaUtilAPI"/>
		<rdfs:comment xml:lang="en">JavaLibrary implementing the java.util package for J2SE 1.2</rdfs:comment>
		<rdfs:comment xml:lang="OWLManchester">platform:comprisesInterfacePart some JavaUtil</rdfs:comment>
	</owl:Class>
	<owl:Class rdf:about="&j2se-1_2;JavaUtilJarAPI">
		<rdfs:subClassOf rdf:resource="&java;JavaAPI"/>
		<rdfs:comment xml:lang="en">JavaLibrary implementing the java.util.jar package for J2SE 1.2</rdfs:comment>
		<rdfs:comment xml:lang="OWLManchester">platform:comprisesInterfacePart some JavaUtilJar</rdfs:comment>
	</owl:Class>
	<owl:Class rdf:about="&j2se-1_2;JavaUtilZipAPI">
		<rdfs:subClassOf rdf:resource="&jdk-1_1;JavaUtilZipAPI"/>
		<rdfs:subClassOf rdf:resource="&personaljava-1_1;JavaUtilZipAPI"/>
		<rdfs:comment xml:lang="en">JavaLibrary implementing the java.util.zip package for J2SE 1.2</rdfs:comment>
		<rdfs:comment xml:lang="OWLManchester">platform:comprisesInterfacePart some JavaUtilZip</rdfs:comment>
	</owl:Class>
	<owl:Class rdf:about="&j2se-1_2;JavaMathAPI">
		<rdfs:subClassOf rdf:resource="&jdk-1_1;JavaMathAPI"/>
		<rdfs:comment xml:lang="en">JavaLibrary implementing the java.math package for J2SE 1.2</rdfs:comment>
		<rdfs:comment xml:lang="OWLManchester">platform:comprisesInterfacePart some JavaMath</rdfs:comment>
	</owl:Class>
	<owl:Class rdf:about="&j2se-1_2;JavaTextAPI">
		<rdfs:subClassOf rdf:resource="&java;JavaAPI"/>
		<rdfs:comment xml:lang="en">JavaLibrary implementing the java.text package for J2SE 1.2</rdfs:comment>
		<rdfs:comment xml:lang="OWLManchester">platform:comprisesInterfacePart some JavaText</rdfs:comment>
	</owl:Class>
	<owl:Class rdf:about="&j2se-1_2;JavaTextResourcesAPI">
		<rdfs:subClassOf rdf:resource="&personaljava-1_1;JavaTextResourcesAPI"/>
		<rdfs:comment xml:lang="en">JavaLibrary implementing the java.text.resources package for J2SE 1.2</rdfs:comment>
		<rdfs:comment xml:lang="OWLManchester">platform:comprisesInterfacePart some JavaTextResources</rdfs:comment>
	</owl:Class>
	<owl:Class rdf:about="&j2se-1_2;JavaAwtAPI">
		<rdfs:subClassOf rdf:resource="&jdk-1_1;JavaAwtAPI"/>
		<rdfs:subClassOf rdf:resource="&personaljava-1_1;JavaAwtAPI"/>
		<rdfs:comment xml:lang="en">JavaLibrary implementing the java.awt package for J2SE 1.2</rdfs:comment>
		<rdfs:comment xml:lang="OWLManchester">platform:comprisesInterfacePart some JavaAwt</rdfs:comment>
	</owl:Class>
	<owl:Class rdf:about="&j2se-1_2;JavaAwtGeomAPI">
		<rdfs:subClassOf rdf:resource="&java;JavaAPI"/>
		<rdfs:comment xml:lang="en">JavaLibrary implementing the java.awt.geom package for J2SE 1.2</rdfs:comment>
		<rdfs:comment xml:lang="OWLManchester">platform:comprisesInterfacePart some JavaAwtGeom</rdfs:comment>
	</owl:Class>
	<owl:Class rdf:about="&j2se-1_2;JavaAwtImageAPI">
		<rdfs:subClassOf rdf:resource="&jdk-1_1;JavaAwtImageAPI"/>
		<rdfs:subClassOf rdf:resource="&personaljava-1_1;JavaAwtImageAPI"/>
		<rdfs:comment xml:lang="en">JavaLibrary implementing the java.awt.image package for J2SE 1.2</rdfs:comment>
		<rdfs:comment xml:lang="OWLManchester">platform:comprisesInterfacePart some JavaAwtImage</rdfs:comment>
	</owl:Class>
	<owl:Class rdf:about="&j2se-1_2;JavaAwtImageRenderableAPI">
		<rdfs:subClassOf rdf:resource="&java;JavaAPI"/>
		<rdfs:comment xml:lang="en">JavaLibrary implementing the java.awt.image.renderable package for J2SE 1.2</rdfs:comment>
		<rdfs:comment xml:lang="OWLManchester">platform:comprisesInterfacePart some JavaAwtImageRenderable</rdfs:comment>
	</owl:Class>
	<owl:Class rdf:about="&j2se-1_2;JavaAwtFontAPI">
		<rdfs:subClassOf rdf:resource="&java;JavaAPI"/>
		<rdfs:comment xml:lang="en">JavaLibrary implementing the java.awt.font package for J2SE 1.2</rdfs:comment>
		<rdfs:comment xml:lang="OWLManchester">platform:comprisesInterfacePart some JavaAwtFont</rdfs:comment>
	</owl:Class>
	<owl:Class rdf:about="&j2se-1_2;JavaAwtEventAPI">
		<rdfs:subClassOf rdf:resource="&jdk-1_1;JavaAwtEventAPI"/>
		<rdfs:subClassOf rdf:resource="&personaljava-1_1;JavaAwtEventAPI"/>
		<rdfs:comment xml:lang="en">JavaLibrary implementing the java.awt.event package for J2SE 1.2</rdfs:comment>
		<rdfs:comment xml:lang="OWLManchester">platform:comprisesInterfacePart some JavaAwtEvent</rdfs:comment>
	</owl:Class>
	<owl:Class rdf:about="&j2se-1_2;JavaAwtDndAPI">
		<rdfs:subClassOf rdf:resource="&java;JavaAPI"/>
		<rdfs:comment xml:lang="en">JavaLibrary implementing the java.awt.dnd package for J2SE 1.2</rdfs:comment>
		<rdfs:comment xml:lang="OWLManchester">platform:comprisesInterfacePart some JavaAwtDnd</rdfs:comment>
	</owl:Class>
	<owl:Class rdf:about="&j2se-1_2;JavaAwtDatatransferAPI">
		<rdfs:subClassOf rdf:resource="&jdk-1_1;JavaAwtDatatransferAPI"/>
		<rdfs:subClassOf rdf:resource="&personaljava-1_1;JavaAwtDatatransferAPI"/>
		<rdfs:comment xml:lang="en">JavaLibrary implementing the java.awt.datatransfer package for J2SE 1.2</rdfs:comment>
		<rdfs:comment xml:lang="OWLManchester">platform:comprisesInterfacePart some JavaAwtDatatransfer</rdfs:comment>
	</owl:Class>
	<owl:Class rdf:about="&j2se-1_2;JavaAwtImAPI">
		<rdfs:subClassOf rdf:resource="&java;JavaAPI"/>
		<rdfs:comment xml:lang="en">JavaLibrary implementing the java.awt.im package for J2SE 1.2</rdfs:comment>
		<rdfs:comment xml:lang="OWLManchester">platform:comprisesInterfacePart some JavaAwtIm</rdfs:comment>
	</owl:Class>
	<owl:Class rdf:about="&j2se-1_2;JavaAwtPrintAPI">
		<rdfs:subClassOf rdf:resource="&java;JavaAPI"/>
		<rdfs:comment xml:lang="en">JavaLibrary implementing the java.awt.print package for J2SE 1.2</rdfs:comment>
		<rdfs:comment xml:lang="OWLManchester">platform:comprisesInterfacePart some JavaAwtPrint</rdfs:comment>
	</owl:Class>
	<owl:Class rdf:about="&j2se-1_2;JavaAwtColorAPI">
		<rdfs:subClassOf rdf:resource="&java;JavaAPI"/>
		<rdfs:comment xml:lang="en">JavaLibrary implementing the java.awt.color package for J2SE 1.2</rdfs:comment>
		<rdfs:comment xml:lang="OWLManchester">platform:comprisesInterfacePart some JavaAwtColor</rdfs:comment>
	</owl:Class>
	<owl:Class rdf:about="&j2se-1_2;JavaBeansAPI">
		<rdfs:subClassOf rdf:resource="&jdk-1_1;JavaBeansAPI"/>
		<rdfs:subClassOf rdf:resource="&personaljava-1_1;JavaBeansAPI"/>
		<rdfs:comment xml:lang="en">JavaLibrary implementing the java.beans package for J2SE 1.2</rdfs:comment>
		<rdfs:comment xml:lang="OWLManchester">platform:comprisesInterfacePart some JavaBeans</rdfs:comment>
	</owl:Class>
	<owl:Class rdf:about="&j2se-1_2;JavaBeansBeancontextAPI">
		<rdfs:subClassOf rdf:resource="&java;JavaAPI"/>
		<rdfs:comment xml:lang="en">JavaLibrary implementing the java.beans.beancontext package for J2SE 1.2</rdfs:comment>
		<rdfs:comment xml:lang="OWLManchester">platform:comprisesInterfacePart some JavaBeansBeancontext</rdfs:comment>
	</owl:Class>
	<owl:Class rdf:about="&j2se-1_2;JavaAppletAPI">
		<rdfs:subClassOf rdf:resource="&jdk-1_1;JavaAppletAPI"/>
		<rdfs:subClassOf rdf:resource="&personaljava-1_1;JavaAppletAPI"/>
		<rdfs:comment xml:lang="en">JavaLibrary implementing the java.applet package for J2SE 1.2</rdfs:comment>
		<rdfs:comment xml:lang="OWLManchester">platform:comprisesInterfacePart some JavaApplet</rdfs:comment>
	</owl:Class>
	<owl:Class rdf:about="&j2se-1_2;JavaRmiAPI">
		<rdfs:subClassOf rdf:resource="&jdk-1_1;JavaRmiAPI"/>
		<rdfs:comment xml:lang="en">JavaLibrary implementing the java.rmi package for J2SE 1.2</rdfs:comment>
		<rdfs:comment xml:lang="OWLManchester">platform:comprisesInterfacePart some JavaRmi</rdfs:comment>
	</owl:Class>
	<owl:Class rdf:about="&j2se-1_2;JavaRmiServerAPI">
		<rdfs:subClassOf rdf:resource="&jdk-1_1;JavaRmiServerAPI"/>
		<rdfs:comment xml:lang="en">JavaLibrary implementing the java.rmi.server package for J2SE 1.2</rdfs:comment>
		<rdfs:comment xml:lang="OWLManchester">platform:comprisesInterfacePart some JavaRmiServer</rdfs:comment>
	</owl:Class>
	<owl:Class rdf:about="&j2se-1_2;JavaRmiDgcAPI">
		<owl:equivalentClass rdf:resource="&jdk-1_1;JavaRmiDgcAPI"/>
		<rdfs:subClassOf rdf:resource="&java;JavaAPI"/>
		<rdfs:comment xml:lang="en">JavaLibrary implementing the java.rmi.dgc package for J2SE 1.2</rdfs:comment>
		<rdfs:comment xml:lang="OWLManchester">platform:comprisesInterfacePart some JavaRmiDgc</rdfs:comment>
	</owl:Class>
	<owl:Class rdf:about="&j2se-1_2;JavaRmiRegistryAPI">
		<rdfs:subClassOf rdf:resource="&jdk-1_1;JavaRmiRegistryAPI"/>
		<rdfs:comment xml:lang="en">JavaLibrary implementing the java.rmi.registry package for J2SE 1.2</rdfs:comment>
		<rdfs:comment xml:lang="OWLManchester">platform:comprisesInterfacePart some JavaRmiRegistry</rdfs:comment>
	</owl:Class>
	<owl:Class rdf:about="&j2se-1_2;JavaRmiActivationAPI">
		<rdfs:subClassOf rdf:resource="&java;JavaAPI"/>
		<rdfs:comment xml:lang="en">JavaLibrary implementing the java.rmi.activation package for J2SE 1.2</rdfs:comment>
		<rdfs:comment xml:lang="OWLManchester">platform:comprisesInterfacePart some JavaRmiActivation</rdfs:comment>
	</owl:Class>
	<owl:Class rdf:about="&j2se-1_2;JavaSqlAPI">
		<rdfs:subClassOf rdf:resource="&jdk-1_1;JavaSqlAPI"/>
		<rdfs:comment xml:lang="en">JavaLibrary implementing the java.sql package for J2SE 1.2</rdfs:comment>
		<rdfs:comment xml:lang="OWLManchester">platform:comprisesInterfacePart some JavaSql</rdfs:comment>
	</owl:Class>
	<owl:Class rdf:about="&j2se-1_2;JavaxSwingAPI">
		<rdfs:subClassOf rdf:resource="&java;JavaAPI"/>
		<rdfs:comment xml:lang="en">JavaLibrary implementing the javax.swing package for J2SE 1.2</rdfs:comment>
		<rdfs:comment xml:lang="OWLManchester">platform:comprisesInterfacePart some JavaxSwing</rdfs:comment>
	</owl:Class>
	<owl:Class rdf:about="&j2se-1_2;JavaxSwingEventAPI">
		<rdfs:subClassOf rdf:resource="&java;JavaAPI"/>
		<rdfs:comment xml:lang="en">JavaLibrary implementing the javax.swing.event package for J2SE 1.2</rdfs:comment>
		<rdfs:comment xml:lang="OWLManchester">platform:comprisesInterfacePart some JavaxSwingEvent</rdfs:comment>
	</owl:Class>
	<owl:Class rdf:about="&j2se-1_2;JavaxSwingTextAPI">
		<rdfs:subClassOf rdf:resource="&java;JavaAPI"/>
		<rdfs:comment xml:lang="en">JavaLibrary implementing the javax.swing.text package for J2SE 1.2</rdfs:comment>
		<rdfs:comment xml:lang="OWLManchester">platform:comprisesInterfacePart some JavaxSwingText</rdfs:comment>
	</owl:Class>
	<owl:Class rdf:about="&j2se-1_2;JavaxSwingTextHtmlAPI">
		<rdfs:subClassOf rdf:resource="&java;JavaAPI"/>
		<rdfs:comment xml:lang="en">JavaLibrary implementing the javax.swing.text.html package for J2SE 1.2</rdfs:comment>
		<rdfs:comment xml:lang="OWLManchester">platform:comprisesInterfacePart some JavaxSwingTextHtml</rdfs:comment>
	</owl:Class>
	<owl:Class rdf:about="&j2se-1_2;JavaxSwingTextHtmlParserAPI">
		<rdfs:subClassOf rdf:resource="&java;JavaAPI"/>
		<rdfs:comment xml:lang="en">JavaLibrary implementing the javax.swing.text.html.parser package for J2SE 1.2</rdfs:comment>
		<rdfs:comment xml:lang="OWLManchester">platform:comprisesInterfacePart some JavaxSwingTextHtmlParser</rdfs:comment>
	</owl:Class>
	<owl:Class rdf:about="&j2se-1_2;JavaxSwingTextRtfAPI">
		<rdfs:subClassOf rdf:resource="&java;JavaAPI"/>
		<rdfs:comment xml:lang="en">JavaLibrary implementing the javax.swing.text.rtf package for J2SE 1.2</rdfs:comment>
		<rdfs:comment xml:lang="OWLManchester">platform:comprisesInterfacePart some JavaxSwingTextRtf</rdfs:comment>
	</owl:Class>
	<owl:Class rdf:about="&j2se-1_2;JavaxSwingUndoAPI">
		<rdfs:subClassOf rdf:resource="&java;JavaAPI"/>
		<rdfs:comment xml:lang="en">JavaLibrary implementing the javax.swing.undo package for J2SE 1.2</rdfs:comment>
		<rdfs:comment xml:lang="OWLManchester">platform:comprisesInterfacePart some JavaxSwingUndo</rdfs:comment>
	</owl:Class>
	<owl:Class rdf:about="&j2se-1_2;JavaxSwingTableAPI">
		<rdfs:subClassOf rdf:resource="&java;JavaAPI"/>
		<rdfs:comment xml:lang="en">JavaLibrary implementing the javax.swing.table package for J2SE 1.2</rdfs:comment>
		<rdfs:comment xml:lang="OWLManchester">platform:comprisesInterfacePart some JavaxSwingTable</rdfs:comment>
	</owl:Class>
	<owl:Class rdf:about="&j2se-1_2;JavaxSwingTreeAPI">
		<rdfs:subClassOf rdf:resource="&java;JavaAPI"/>
		<rdfs:comment xml:lang="en">JavaLibrary implementing the javax.swing.tree package for J2SE 1.2</rdfs:comment>
		<rdfs:comment xml:lang="OWLManchester">platform:comprisesInterfacePart some JavaxSwingTree</rdfs:comment>
	</owl:Class>
	<owl:Class rdf:about="&j2se-1_2;JavaxSwingPlafAPI">
		<rdfs:subClassOf rdf:resource="&java;JavaAPI"/>
		<rdfs:comment xml:lang="en">JavaLibrary implementing the javax.swing.plaf package for J2SE 1.2</rdfs:comment>
		<rdfs:comment xml:lang="OWLManchester">platform:comprisesInterfacePart some JavaxSwingPlaf</rdfs:comment>
	</owl:Class>
	<owl:Class rdf:about="&j2se-1_2;JavaxSwingPlafBasicAPI">
		<rdfs:subClassOf rdf:resource="&java;JavaAPI"/>
		<rdfs:comment xml:lang="en">JavaLibrary implementing the javax.swing.plaf.basic package for J2SE 1.2</rdfs:comment>
		<rdfs:comment xml:lang="OWLManchester">platform:comprisesInterfacePart some JavaxSwingPlafBasic</rdfs:comment>
	</owl:Class>
	<owl:Class rdf:about="&j2se-1_2;JavaxSwingPlafMetalAPI">
		<rdfs:subClassOf rdf:resource="&java;JavaAPI"/>
		<rdfs:comment xml:lang="en">JavaLibrary implementing the javax.swing.plaf.metal package for J2SE 1.2</rdfs:comment>
		<rdfs:comment xml:lang="OWLManchester">platform:comprisesInterfacePart some JavaxSwingPlafMetal</rdfs:comment>
	</owl:Class>
	<owl:Class rdf:about="&j2se-1_2;JavaxSwingPlafMultiAPI">
		<rdfs:subClassOf rdf:resource="&java;JavaAPI"/>
		<rdfs:comment xml:lang="en">JavaLibrary implementing the javax.swing.plaf.multi package for J2SE 1.2</rdfs:comment>
		<rdfs:comment xml:lang="OWLManchester">platform:comprisesInterfacePart some JavaxSwingPlafMulti</rdfs:comment>
	</owl:Class>
	<owl:Class rdf:about="&j2se-1_2;JavaxSwingBorderAPI">
		<rdfs:subClassOf rdf:resource="&java;JavaAPI"/>
		<rdfs:comment xml:lang="en">JavaLibrary implementing the javax.swing.border package for J2SE 1.2</rdfs:comment>
		<rdfs:comment xml:lang="OWLManchester">platform:comprisesInterfacePart some JavaxSwingBorder</rdfs:comment>
	</owl:Class>
	<owl:Class rdf:about="&j2se-1_2;JavaxSwingColorchooserAPI">
		<rdfs:subClassOf rdf:resource="&java;JavaAPI"/>
		<rdfs:comment xml:lang="en">JavaLibrary implementing the javax.swing.colorchooser package for J2SE 1.2</rdfs:comment>
		<rdfs:comment xml:lang="OWLManchester">platform:comprisesInterfacePart some JavaxSwingColorchooser</rdfs:comment>
	</owl:Class>
	<owl:Class rdf:about="&j2se-1_2;JavaxSwingFilechooserAPI">
		<rdfs:subClassOf rdf:resource="&java;JavaAPI"/>
		<rdfs:comment xml:lang="en">JavaLibrary implementing the javax.swing.filechooser package for J2SE 1.2</rdfs:comment>
		<rdfs:comment xml:lang="OWLManchester">platform:comprisesInterfacePart some JavaxSwingFilechooser</rdfs:comment>
	</owl:Class>
	<owl:Class rdf:about="&j2se-1_2;JavaxAccessibilityAPI">
		<rdfs:subClassOf rdf:resource="&java;JavaAPI"/>
		<rdfs:comment xml:lang="en">JavaLibrary implementing the javax.accessibility package for J2SE 1.2</rdfs:comment>
		<rdfs:comment xml:lang="OWLManchester">platform:comprisesInterfacePart some JavaxAccessibility</rdfs:comment>
	</owl:Class>
	<owl:Class rdf:about="&j2se-1_2;OrgOmgCORBAAPI">
		<rdfs:subClassOf rdf:resource="&java;JavaAPI"/>
		<rdfs:comment xml:lang="en">JavaLibrary implementing the org.omg.CORBA package for J2SE 1.2</rdfs:comment>
		<rdfs:comment xml:lang="OWLManchester">platform:comprisesInterfacePart some OrgOmgCORBA</rdfs:comment>
	</owl:Class>
	<owl:Class rdf:about="&j2se-1_2;OrgOmgCORBAPortableAPI">
		<rdfs:subClassOf rdf:resource="&java;JavaAPI"/>
		<rdfs:comment xml:lang="en">JavaLibrary implementing the org.omg.CORBA.portable package for J2SE 1.2</rdfs:comment>
		<rdfs:comment xml:lang="OWLManchester">platform:comprisesInterfacePart some OrgOmgCORBAPortable</rdfs:comment>
	</owl:Class>
	<owl:Class rdf:about="&j2se-1_2;OrgOmgCORBADynAnyPackageAPI">
		<rdfs:subClassOf rdf:resource="&java;JavaAPI"/>
		<rdfs:comment xml:lang="en">JavaLibrary implementing the org.omg.CORBA.DynAnyPackage package for J2SE 1.2</rdfs:comment>
		<rdfs:comment xml:lang="OWLManchester">platform:comprisesInterfacePart some OrgOmgCORBADynAnyPackage</rdfs:comment>
	</owl:Class>
	<owl:Class rdf:about="&j2se-1_2;OrgOmgCORBAORBPackageAPI">
		<rdfs:subClassOf rdf:resource="&java;JavaAPI"/>
		<rdfs:comment xml:lang="en">JavaLibrary implementing the org.omg.CORBA.ORBPackage package for J2SE 1.2</rdfs:comment>
		<rdfs:comment xml:lang="OWLManchester">platform:comprisesInterfacePart some OrgOmgCORBAORBPackage</rdfs:comment>
	</owl:Class>
	<owl:Class rdf:about="&j2se-1_2;OrgOmgCORBATypeCodePackageAPI">
		<rdfs:subClassOf rdf:resource="&java;JavaAPI"/>
		<rdfs:comment xml:lang="en">JavaLibrary implementing the org.omg.CORBA.TypeCodePackage package for J2SE 1.2</rdfs:comment>
		<rdfs:comment xml:lang="OWLManchester">platform:comprisesInterfacePart some OrgOmgCORBATypeCodePackage</rdfs:comment>
	</owl:Class>
	<owl:Class rdf:about="&j2se-1_2;OrgOmgCosNamingAPI">
		<rdfs:subClassOf rdf:resource="&java;JavaAPI"/>
		<rdfs:comment xml:lang="en">JavaLibrary implementing the org.omg.CosNaming package for J2SE 1.2</rdfs:comment>
		<rdfs:comment xml:lang="OWLManchester">platform:comprisesInterfacePart some OrgOmgCosNaming</rdfs:comment>
	</owl:Class>
	<owl:Class rdf:about="&j2se-1_2;OrgOmgCosNamingNamingContextPackageAPI">
		<rdfs:subClassOf rdf:resource="&java;JavaAPI"/>
		<rdfs:comment xml:lang="en">JavaLibrary implementing the org.omg.CosNaming.NamingContextPackage package for J2SE 1.2</rdfs:comment>
		<rdfs:comment xml:lang="OWLManchester">platform:comprisesInterfacePart some OrgOmgCosNamingNamingContextPackage</rdfs:comment>
	</owl:Class>
	<j2se-1_2:JavaIo rdf:about="&j2se-1_2;theJavaIoPart">
	</j2se-1_2:JavaIo>
	<j2se-1_2:JavaLang rdf:about="&j2se-1_2;theJavaLangPart">
	</j2se-1_2:JavaLang>
	<j2se-1_2:JavaLangReflect rdf:about="&j2se-1_2;theJavaLangReflectPart">
	</j2se-1_2:JavaLangReflect>
	<j2se-1_2:JavaLangRef rdf:about="&j2se-1_2;theJavaLangRefPart">
	</j2se-1_2:JavaLangRef>
	<j2se-1_2:JavaNet rdf:about="&j2se-1_2;theJavaNetPart">
	</j2se-1_2:JavaNet>
	<j2se-1_2:JavaSecurity rdf:about="&j2se-1_2;theJavaSecurityPart">
	</j2se-1_2:JavaSecurity>
	<j2se-1_2:JavaSecurityCert rdf:about="&j2se-1_2;theJavaSecurityCertPart">
	</j2se-1_2:JavaSecurityCert>
	<j2se-1_2:JavaSecuritySpec rdf:about="&j2se-1_2;theJavaSecuritySpecPart">
	</j2se-1_2:JavaSecuritySpec>
	<j2se-1_2:JavaSecurityInterfaces rdf:about="&j2se-1_2;theJavaSecurityInterfacesPart">
	</j2se-1_2:JavaSecurityInterfaces>
	<j2se-1_2:JavaSecurityAcl rdf:about="&j2se-1_2;theJavaSecurityAclPart">
	</j2se-1_2:JavaSecurityAcl>
	<j2se-1_2:JavaUtil rdf:about="&j2se-1_2;theJavaUtilPart">
	</j2se-1_2:JavaUtil>
	<j2se-1_2:JavaUtilJar rdf:about="&j2se-1_2;theJavaUtilJarPart">
	</j2se-1_2:JavaUtilJar>
	<j2se-1_2:JavaUtilZip rdf:about="&j2se-1_2;theJavaUtilZipPart">
	</j2se-1_2:JavaUtilZip>
	<j2se-1_2:JavaMath rdf:about="&j2se-1_2;theJavaMathPart">
	</j2se-1_2:JavaMath>
	<j2se-1_2:JavaText rdf:about="&j2se-1_2;theJavaTextPart">
	</j2se-1_2:JavaText>
	<j2se-1_2:JavaTextResources rdf:about="&j2se-1_2;theJavaTextResourcesPart">
	</j2se-1_2:JavaTextResources>
	<j2se-1_2:JavaAwt rdf:about="&j2se-1_2;theJavaAwtPart">
	</j2se-1_2:JavaAwt>
	<j2se-1_2:JavaAwtGeom rdf:about="&j2se-1_2;theJavaAwtGeomPart">
	</j2se-1_2:JavaAwtGeom>
	<j2se-1_2:JavaAwtImage rdf:about="&j2se-1_2;theJavaAwtImagePart">
	</j2se-1_2:JavaAwtImage>
	<j2se-1_2:JavaAwtImageRenderable rdf:about="&j2se-1_2;theJavaAwtImageRenderablePart">
	</j2se-1_2:JavaAwtImageRenderable>
	<j2se-1_2:JavaAwtFont rdf:about="&j2se-1_2;theJavaAwtFontPart">
	</j2se-1_2:JavaAwtFont>
	<j2se-1_2:JavaAwtEvent rdf:about="&j2se-1_2;theJavaAwtEventPart">
	</j2se-1_2:JavaAwtEvent>
	<j2se-1_2:JavaAwtDnd rdf:about="&j2se-1_2;theJavaAwtDndPart">
	</j2se-1_2:JavaAwtDnd>
	<j2se-1_2:JavaAwtDatatransfer rdf:about="&j2se-1_2;theJavaAwtDatatransferPart">
	</j2se-1_2:JavaAwtDatatransfer>
	<j2se-1_2:JavaAwtIm rdf:about="&j2se-1_2;theJavaAwtImPart">
	</j2se-1_2:JavaAwtIm>
	<j2se-1_2:JavaAwtPrint rdf:about="&j2se-1_2;theJavaAwtPrintPart">
	</j2se-1_2:JavaAwtPrint>
	<j2se-1_2:JavaAwtColor rdf:about="&j2se-1_2;theJavaAwtColorPart">
	</j2se-1_2:JavaAwtColor>
	<j2se-1_2:JavaBeans rdf:about="&j2se-1_2;theJavaBeansPart">
	</j2se-1_2:JavaBeans>
	<j2se-1_2:JavaBeansBeancontext rdf:about="&j2se-1_2;theJavaBeansBeancontextPart">
	</j2se-1_2:JavaBeansBeancontext>
	<j2se-1_2:JavaApplet rdf:about="&j2se-1_2;theJavaAppletPart">
	</j2se-1_2:JavaApplet>
	<j2se-1_2:JavaRmi rdf:about="&j2se-1_2;theJavaRmiPart">
	</j2se-1_2:JavaRmi>
	<j2se-1_2:JavaRmiServer rdf:about="&j2se-1_2;theJavaRmiServerPart">
	</j2se-1_2:JavaRmiServer>
	<j2se-1_2:JavaRmiDgc rdf:about="&j2se-1_2;theJavaRmiDgcPart">
	</j2se-1_2:JavaRmiDgc>
	<j2se-1_2:JavaRmiRegistry rdf:about="&j2se-1_2;theJavaRmiRegistryPart">
	</j2se-1_2:JavaRmiRegistry>
	<j2se-1_2:JavaRmiActivation rdf:about="&j2se-1_2;theJavaRmiActivationPart">
	</j2se-1_2:JavaRmiActivation>
	<j2se-1_2:JavaSql rdf:about="&j2se-1_2;theJavaSqlPart">
	</j2se-1_2:JavaSql>
	<j2se-1_2:JavaxSwing rdf:about="&j2se-1_2;theJavaxSwingPart">
	</j2se-1_2:JavaxSwing>
	<j2se-1_2:JavaxSwingEvent rdf:about="&j2se-1_2;theJavaxSwingEventPart">
	</j2se-1_2:JavaxSwingEvent>
	<j2se-1_2:JavaxSwingText rdf:about="&j2se-1_2;theJavaxSwingTextPart">
	</j2se-1_2:JavaxSwingText>
	<j2se-1_2:JavaxSwingTextHtml rdf:about="&j2se-1_2;theJavaxSwingTextHtmlPart">
	</j2se-1_2:JavaxSwingTextHtml>
	<j2se-1_2:JavaxSwingTextHtmlParser rdf:about="&j2se-1_2;theJavaxSwingTextHtmlParserPart">
	</j2se-1_2:JavaxSwingTextHtmlParser>
	<j2se-1_2:JavaxSwingTextRtf rdf:about="&j2se-1_2;theJavaxSwingTextRtfPart">
	</j2se-1_2:JavaxSwingTextRtf>
	<j2se-1_2:JavaxSwingUndo rdf:about="&j2se-1_2;theJavaxSwingUndoPart">
	</j2se-1_2:JavaxSwingUndo>
	<j2se-1_2:JavaxSwingTable rdf:about="&j2se-1_2;theJavaxSwingTablePart">
	</j2se-1_2:JavaxSwingTable>
	<j2se-1_2:JavaxSwingTree rdf:about="&j2se-1_2;theJavaxSwingTreePart">
	</j2se-1_2:JavaxSwingTree>
	<j2se-1_2:JavaxSwingPlaf rdf:about="&j2se-1_2;theJavaxSwingPlafPart">
	</j2se-1_2:JavaxSwingPlaf>
	<j2se-1_2:JavaxSwingPlafBasic rdf:about="&j2se-1_2;theJavaxSwingPlafBasicPart">
	</j2se-1_2:JavaxSwingPlafBasic>
	<j2se-1_2:JavaxSwingPlafMetal rdf:about="&j2se-1_2;theJavaxSwingPlafMetalPart">
	</j2se-1_2:JavaxSwingPlafMetal>
	<j2se-1_2:JavaxSwingPlafMulti rdf:about="&j2se-1_2;theJavaxSwingPlafMultiPart">
	</j2se-1_2:JavaxSwingPlafMulti>
	<j2se-1_2:JavaxSwingBorder rdf:about="&j2se-1_2;theJavaxSwingBorderPart">
	</j2se-1_2:JavaxSwingBorder>
	<j2se-1_2:JavaxSwingColorchooser rdf:about="&j2se-1_2;theJavaxSwingColorchooserPart">
	</j2se-1_2:JavaxSwingColorchooser>
	<j2se-1_2:JavaxSwingFilechooser rdf:about="&j2se-1_2;theJavaxSwingFilechooserPart">
	</j2se-1_2:JavaxSwingFilechooser>
	<j2se-1_2:JavaxAccessibility rdf:about="&j2se-1_2;theJavaxAccessibilityPart">
	</j2se-1_2:JavaxAccessibility>
	<j2se-1_2:OrgOmgCORBA rdf:about="&j2se-1_2;theOrgOmgCORBAPart">
	</j2se-1_2:OrgOmgCORBA>
	<j2se-1_2:OrgOmgCORBAPortable rdf:about="&j2se-1_2;theOrgOmgCORBAPortablePart">
	</j2se-1_2:OrgOmgCORBAPortable>
	<j2se-1_2:OrgOmgCORBADynAnyPackage rdf:about="&j2se-1_2;theOrgOmgCORBADynAnyPackagePart">
	</j2se-1_2:OrgOmgCORBADynAnyPackage>
	<j2se-1_2:OrgOmgCORBAORBPackage rdf:about="&j2se-1_2;theOrgOmgCORBAORBPackagePart">
	</j2se-1_2:OrgOmgCORBAORBPackage>
	<j2se-1_2:OrgOmgCORBATypeCodePackage rdf:about="&j2se-1_2;theOrgOmgCORBATypeCodePackagePart">
	</j2se-1_2:OrgOmgCORBATypeCodePackage>
	<j2se-1_2:OrgOmgCosNaming rdf:about="&j2se-1_2;theOrgOmgCosNamingPart">
	</j2se-1_2:OrgOmgCosNaming>
	<j2se-1_2:OrgOmgCosNamingNamingContextPackage rdf:about="&j2se-1_2;theOrgOmgCosNamingNamingContextPackagePart">
	</j2se-1_2:OrgOmgCosNamingNamingContextPackage>
	<owl:Class rdf:about="&j2se-1_2;JavaIoClassLibrary">
		<rdfs:subClassOf rdf:resource="&jdk-1_1;JavaIoClassLibrary"/>
		<rdfs:subClassOf rdf:resource="&j2me-midp-2_0;JavaIoClassLibrary"/>
		<rdfs:subClassOf rdf:resource="&personaljava-1_1;JavaIoClassLibrary"/>
		<rdfs:comment xml:lang="en">JavaLibrary implementing the java.io package for J2SE 1.2</rdfs:comment>
		<rdfs:comment xml:lang="OWLManchester">platform:implementsInterface some JavaIoAPI</rdfs:comment>
	</owl:Class>
	<owl:Class rdf:about="&j2se-1_2;JavaLangClassLibrary">
		<rdfs:subClassOf rdf:resource="&j2me-midp-2_0;JavaLangClassLibrary"/>
		<rdfs:comment xml:lang="en">JavaLibrary implementing the java.lang package for J2SE 1.2</rdfs:comment>
		<rdfs:comment xml:lang="OWLManchester">platform:implementsInterface some JavaLangAPI</rdfs:comment>
	</owl:Class>
	<owl:Class rdf:about="&j2se-1_2;JavaLangReflectClassLibrary">
		<rdfs:subClassOf rdf:resource="&jdk-1_1;JavaLangReflectClassLibrary"/>
		<rdfs:subClassOf rdf:resource="&personaljava-1_1;JavaLangReflectClassLibrary"/>
		<rdfs:comment xml:lang="en">JavaLibrary implementing the java.lang.reflect package for J2SE 1.2</rdfs:comment>
		<rdfs:comment xml:lang="OWLManchester">platform:implementsInterface some JavaLangReflectAPI</rdfs:comment>
	</owl:Class>
	<owl:Class rdf:about="&j2se-1_2;JavaLangRefClassLibrary">
		<rdfs:subClassOf rdf:resource="&java;JavaClassLibrary"/>
		<rdfs:comment xml:lang="en">JavaLibrary implementing the java.lang.ref package for J2SE 1.2</rdfs:comment>
		<rdfs:comment xml:lang="OWLManchester">platform:implementsInterface some JavaLangRefAPI</rdfs:comment>
	</owl:Class>
	<owl:Class rdf:about="&j2se-1_2;JavaNetClassLibrary">
		<rdfs:subClassOf rdf:resource="&jdk-1_1;JavaNetClassLibrary"/>
		<rdfs:subClassOf rdf:resource="&personaljava-1_1;JavaNetClassLibrary"/>
		<rdfs:comment xml:lang="en">JavaLibrary implementing the java.net package for J2SE 1.2</rdfs:comment>
		<rdfs:comment xml:lang="OWLManchester">platform:implementsInterface some JavaNetAPI</rdfs:comment>
	</owl:Class>
	<owl:Class rdf:about="&j2se-1_2;JavaSecurityClassLibrary">
		<rdfs:subClassOf rdf:resource="&jdk-1_1;JavaSecurityClassLibrary"/>
		<rdfs:comment xml:lang="en">JavaLibrary implementing the java.security package for J2SE 1.2</rdfs:comment>
		<rdfs:comment xml:lang="OWLManchester">platform:implementsInterface some JavaSecurityAPI</rdfs:comment>
	</owl:Class>
	<owl:Class rdf:about="&j2se-1_2;JavaSecurityCertClassLibrary">
		<rdfs:subClassOf rdf:resource="&java;JavaClassLibrary"/>
		<rdfs:comment xml:lang="en">JavaLibrary implementing the java.security.cert package for J2SE 1.2</rdfs:comment>
		<rdfs:comment xml:lang="OWLManchester">platform:implementsInterface some JavaSecurityCertAPI</rdfs:comment>
	</owl:Class>
	<owl:Class rdf:about="&j2se-1_2;JavaSecuritySpecClassLibrary">
		<rdfs:subClassOf rdf:resource="&java;JavaClassLibrary"/>
		<rdfs:comment xml:lang="en">JavaLibrary implementing the java.security.spec package for J2SE 1.2</rdfs:comment>
		<rdfs:comment xml:lang="OWLManchester">platform:implementsInterface some JavaSecuritySpecAPI</rdfs:comment>
	</owl:Class>
	<owl:Class rdf:about="&j2se-1_2;JavaSecurityInterfacesClassLibrary">
		<rdfs:subClassOf rdf:resource="&jdk-1_1;JavaSecurityInterfacesClassLibrary"/>
		<rdfs:comment xml:lang="en">JavaLibrary implementing the java.security.interfaces package for J2SE 1.2</rdfs:comment>
		<rdfs:comment xml:lang="OWLManchester">platform:implementsInterface some JavaSecurityInterfacesAPI</rdfs:comment>
	</owl:Class>
	<owl:Class rdf:about="&j2se-1_2;JavaSecurityAclClassLibrary">
		<owl:equivalentClass rdf:resource="&jdk-1_1;JavaSecurityAclClassLibrary"/>
		<rdfs:subClassOf rdf:resource="&java;JavaClassLibrary"/>
		<rdfs:comment xml:lang="en">JavaLibrary implementing the java.security.acl package for J2SE 1.2</rdfs:comment>
		<rdfs:comment xml:lang="OWLManchester">platform:implementsInterface some JavaSecurityAclAPI</rdfs:comment>
	</owl:Class>
	<owl:Class rdf:about="&j2se-1_2;JavaUtilClassLibrary">
		<rdfs:subClassOf rdf:resource="&jdk-1_1;JavaUtilClassLibrary"/>
		<rdfs:subClassOf rdf:resource="&personaljava-1_1;JavaUtilClassLibrary"/>
		<rdfs:comment xml:lang="en">JavaLibrary implementing the java.util package for J2SE 1.2</rdfs:comment>
		<rdfs:comment xml:lang="OWLManchester">platform:implementsInterface some JavaUtilAPI</rdfs:comment>
	</owl:Class>
	<owl:Class rdf:about="&j2se-1_2;JavaUtilJarClassLibrary">
		<rdfs:subClassOf rdf:resource="&java;JavaClassLibrary"/>
		<rdfs:comment xml:lang="en">JavaLibrary implementing the java.util.jar package for J2SE 1.2</rdfs:comment>
		<rdfs:comment xml:lang="OWLManchester">platform:implementsInterface some JavaUtilJarAPI</rdfs:comment>
	</owl:Class>
	<owl:Class rdf:about="&j2se-1_2;JavaUtilZipClassLibrary">
		<rdfs:subClassOf rdf:resource="&jdk-1_1;JavaUtilZipClassLibrary"/>
		<rdfs:subClassOf rdf:resource="&personaljava-1_1;JavaUtilZipClassLibrary"/>
		<rdfs:comment xml:lang="en">JavaLibrary implementing the java.util.zip package for J2SE 1.2</rdfs:comment>
		<rdfs:comment xml:lang="OWLManchester">platform:implementsInterface some JavaUtilZipAPI</rdfs:comment>
	</owl:Class>
	<owl:Class rdf:about="&j2se-1_2;JavaMathClassLibrary">
		<rdfs:subClassOf rdf:resource="&jdk-1_1;JavaMathClassLibrary"/>
		<rdfs:comment xml:lang="en">JavaLibrary implementing the java.math package for J2SE 1.2</rdfs:comment>
		<rdfs:comment xml:lang="OWLManchester">platform:implementsInterface some JavaMathAPI</rdfs:comment>
	</owl:Class>
	<owl:Class rdf:about="&j2se-1_2;JavaTextClassLibrary">
		<rdfs:subClassOf rdf:resource="&java;JavaClassLibrary"/>
		<rdfs:comment xml:lang="en">JavaLibrary implementing the java.text package for J2SE 1.2</rdfs:comment>
		<rdfs:comment xml:lang="OWLManchester">platform:implementsInterface some JavaTextAPI</rdfs:comment>
	</owl:Class>
	<owl:Class rdf:about="&j2se-1_2;JavaTextResourcesClassLibrary">
		<rdfs:subClassOf rdf:resource="&personaljava-1_1;JavaTextResourcesClassLibrary"/>
		<rdfs:comment xml:lang="en">JavaLibrary implementing the java.text.resources package for J2SE 1.2</rdfs:comment>
		<rdfs:comment xml:lang="OWLManchester">platform:implementsInterface some JavaTextResourcesAPI</rdfs:comment>
	</owl:Class>
	<owl:Class rdf:about="&j2se-1_2;JavaAwtClassLibrary">
		<rdfs:subClassOf rdf:resource="&jdk-1_1;JavaAwtClassLibrary"/>
		<rdfs:subClassOf rdf:resource="&personaljava-1_1;JavaAwtClassLibrary"/>
		<rdfs:comment xml:lang="en">JavaLibrary implementing the java.awt package for J2SE 1.2</rdfs:comment>
		<rdfs:comment xml:lang="OWLManchester">platform:implementsInterface some JavaAwtAPI</rdfs:comment>
	</owl:Class>
	<owl:Class rdf:about="&j2se-1_2;JavaAwtGeomClassLibrary">
		<rdfs:subClassOf rdf:resource="&java;JavaClassLibrary"/>
		<rdfs:comment xml:lang="en">JavaLibrary implementing the java.awt.geom package for J2SE 1.2</rdfs:comment>
		<rdfs:comment xml:lang="OWLManchester">platform:implementsInterface some JavaAwtGeomAPI</rdfs:comment>
	</owl:Class>
	<owl:Class rdf:about="&j2se-1_2;JavaAwtImageClassLibrary">
		<rdfs:subClassOf rdf:resource="&jdk-1_1;JavaAwtImageClassLibrary"/>
		<rdfs:subClassOf rdf:resource="&personaljava-1_1;JavaAwtImageClassLibrary"/>
		<rdfs:comment xml:lang="en">JavaLibrary implementing the java.awt.image package for J2SE 1.2</rdfs:comment>
		<rdfs:comment xml:lang="OWLManchester">platform:implementsInterface some JavaAwtImageAPI</rdfs:comment>
	</owl:Class>
	<owl:Class rdf:about="&j2se-1_2;JavaAwtImageRenderableClassLibrary">
		<rdfs:subClassOf rdf:resource="&java;JavaClassLibrary"/>
		<rdfs:comment xml:lang="en">JavaLibrary implementing the java.awt.image.renderable package for J2SE 1.2</rdfs:comment>
		<rdfs:comment xml:lang="OWLManchester">platform:implementsInterface some JavaAwtImageRenderableAPI</rdfs:comment>
	</owl:Class>
	<owl:Class rdf:about="&j2se-1_2;JavaAwtFontClassLibrary">
		<rdfs:subClassOf rdf:resource="&java;JavaClassLibrary"/>
		<rdfs:comment xml:lang="en">JavaLibrary implementing the java.awt.font package for J2SE 1.2</rdfs:comment>
		<rdfs:comment xml:lang="OWLManchester">platform:implementsInterface some JavaAwtFontAPI</rdfs:comment>
	</owl:Class>
	<owl:Class rdf:about="&j2se-1_2;JavaAwtEventClassLibrary">
		<rdfs:subClassOf rdf:resource="&jdk-1_1;JavaAwtEventClassLibrary"/>
		<rdfs:subClassOf rdf:resource="&personaljava-1_1;JavaAwtEventClassLibrary"/>
		<rdfs:comment xml:lang="en">JavaLibrary implementing the java.awt.event package for J2SE 1.2</rdfs:comment>
		<rdfs:comment xml:lang="OWLManchester">platform:implementsInterface some JavaAwtEventAPI</rdfs:comment>
	</owl:Class>
	<owl:Class rdf:about="&j2se-1_2;JavaAwtDndClassLibrary">
		<rdfs:subClassOf rdf:resource="&java;JavaClassLibrary"/>
		<rdfs:comment xml:lang="en">JavaLibrary implementing the java.awt.dnd package for J2SE 1.2</rdfs:comment>
		<rdfs:comment xml:lang="OWLManchester">platform:implementsInterface some JavaAwtDndAPI</rdfs:comment>
	</owl:Class>
	<owl:Class rdf:about="&j2se-1_2;JavaAwtDatatransferClassLibrary">
		<rdfs:subClassOf rdf:resource="&jdk-1_1;JavaAwtDatatransferClassLibrary"/>
		<rdfs:subClassOf rdf:resource="&personaljava-1_1;JavaAwtDatatransferClassLibrary"/>
		<rdfs:comment xml:lang="en">JavaLibrary implementing the java.awt.datatransfer package for J2SE 1.2</rdfs:comment>
		<rdfs:comment xml:lang="OWLManchester">platform:implementsInterface some JavaAwtDatatransferAPI</rdfs:comment>
	</owl:Class>
	<owl:Class rdf:about="&j2se-1_2;JavaAwtImClassLibrary">
		<rdfs:subClassOf rdf:resource="&java;JavaClassLibrary"/>
		<rdfs:comment xml:lang="en">JavaLibrary implementing the java.awt.im package for J2SE 1.2</rdfs:comment>
		<rdfs:comment xml:lang="OWLManchester">platform:implementsInterface some JavaAwtImAPI</rdfs:comment>
	</owl:Class>
	<owl:Class rdf:about="&j2se-1_2;JavaAwtPrintClassLibrary">
		<rdfs:subClassOf rdf:resource="&java;JavaClassLibrary"/>
		<rdfs:comment xml:lang="en">JavaLibrary implementing the java.awt.print package for J2SE 1.2</rdfs:comment>
		<rdfs:comment xml:lang="OWLManchester">platform:implementsInterface some JavaAwtPrintAPI</rdfs:comment>
	</owl:Class>
	<owl:Class rdf:about="&j2se-1_2;JavaAwtColorClassLibrary">
		<rdfs:subClassOf rdf:resource="&java;JavaClassLibrary"/>
		<rdfs:comment xml:lang="en">JavaLibrary implementing the java.awt.color package for J2SE 1.2</rdfs:comment>
		<rdfs:comment xml:lang="OWLManchester">platform:implementsInterface some JavaAwtColorAPI</rdfs:comment>
	</owl:Class>
	<owl:Class rdf:about="&j2se-1_2;JavaBeansClassLibrary">
		<rdfs:subClassOf rdf:resource="&jdk-1_1;JavaBeansClassLibrary"/>
		<rdfs:subClassOf rdf:resource="&personaljava-1_1;JavaBeansClassLibrary"/>
		<rdfs:comment xml:lang="en">JavaLibrary implementing the java.beans package for J2SE 1.2</rdfs:comment>
		<rdfs:comment xml:lang="OWLManchester">platform:implementsInterface some JavaBeansAPI</rdfs:comment>
	</owl:Class>
	<owl:Class rdf:about="&j2se-1_2;JavaBeansBeancontextClassLibrary">
		<rdfs:subClassOf rdf:resource="&java;JavaClassLibrary"/>
		<rdfs:comment xml:lang="en">JavaLibrary implementing the java.beans.beancontext package for J2SE 1.2</rdfs:comment>
		<rdfs:comment xml:lang="OWLManchester">platform:implementsInterface some JavaBeansBeancontextAPI</rdfs:comment>
	</owl:Class>
	<owl:Class rdf:about="&j2se-1_2;JavaAppletClassLibrary">
		<rdfs:subClassOf rdf:resource="&jdk-1_1;JavaAppletClassLibrary"/>
		<rdfs:subClassOf rdf:resource="&personaljava-1_1;JavaAppletClassLibrary"/>
		<rdfs:comment xml:lang="en">JavaLibrary implementing the java.applet package for J2SE 1.2</rdfs:comment>
		<rdfs:comment xml:lang="OWLManchester">platform:implementsInterface some JavaAppletAPI</rdfs:comment>
	</owl:Class>
	<owl:Class rdf:about="&j2se-1_2;JavaRmiClassLibrary">
		<rdfs:subClassOf rdf:resource="&jdk-1_1;JavaRmiClassLibrary"/>
		<rdfs:comment xml:lang="en">JavaLibrary implementing the java.rmi package for J2SE 1.2</rdfs:comment>
		<rdfs:comment xml:lang="OWLManchester">platform:implementsInterface some JavaRmiAPI</rdfs:comment>
	</owl:Class>
	<owl:Class rdf:about="&j2se-1_2;JavaRmiServerClassLibrary">
		<rdfs:subClassOf rdf:resource="&jdk-1_1;JavaRmiServerClassLibrary"/>
		<rdfs:comment xml:lang="en">JavaLibrary implementing the java.rmi.server package for J2SE 1.2</rdfs:comment>
		<rdfs:comment xml:lang="OWLManchester">platform:implementsInterface some JavaRmiServerAPI</rdfs:comment>
	</owl:Class>
	<owl:Class rdf:about="&j2se-1_2;JavaRmiDgcClassLibrary">
		<owl:equivalentClass rdf:resource="&jdk-1_1;JavaRmiDgcClassLibrary"/>
		<rdfs:subClassOf rdf:resource="&java;JavaClassLibrary"/>
		<rdfs:comment xml:lang="en">JavaLibrary implementing the java.rmi.dgc package for J2SE 1.2</rdfs:comment>
		<rdfs:comment xml:lang="OWLManchester">platform:implementsInterface some JavaRmiDgcAPI</rdfs:comment>
	</owl:Class>
	<owl:Class rdf:about="&j2se-1_2;JavaRmiRegistryClassLibrary">
		<rdfs:subClassOf rdf:resource="&jdk-1_1;JavaRmiRegistryClassLibrary"/>
		<rdfs:comment xml:lang="en">JavaLibrary implementing the java.rmi.registry package for J2SE 1.2</rdfs:comment>
		<rdfs:comment xml:lang="OWLManchester">platform:implementsInterface some JavaRmiRegistryAPI</rdfs:comment>
	</owl:Class>
	<owl:Class rdf:about="&j2se-1_2;JavaRmiActivationClassLibrary">
		<rdfs:subClassOf rdf:resource="&java;JavaClassLibrary"/>
		<rdfs:comment xml:lang="en">JavaLibrary implementing the java.rmi.activation package for J2SE 1.2</rdfs:comment>
		<rdfs:comment xml:lang="OWLManchester">platform:implementsInterface some JavaRmiActivationAPI</rdfs:comment>
	</owl:Class>
	<owl:Class rdf:about="&j2se-1_2;JavaSqlClassLibrary">
		<rdfs:subClassOf rdf:resource="&jdk-1_1;JavaSqlClassLibrary"/>
		<rdfs:comment xml:lang="en">JavaLibrary implementing the java.sql package for J2SE 1.2</rdfs:comment>
		<rdfs:comment xml:lang="OWLManchester">platform:implementsInterface some JavaSqlAPI</rdfs:comment>
	</owl:Class>
	<owl:Class rdf:about="&j2se-1_2;JavaxSwingClassLibrary">
		<rdfs:subClassOf rdf:resource="&java;JavaClassLibrary"/>
		<rdfs:comment xml:lang="en">JavaLibrary implementing the javax.swing package for J2SE 1.2</rdfs:comment>
		<rdfs:comment xml:lang="OWLManchester">platform:implementsInterface some JavaxSwingAPI</rdfs:comment>
	</owl:Class>
	<owl:Class rdf:about="&j2se-1_2;JavaxSwingEventClassLibrary">
		<rdfs:subClassOf rdf:resource="&java;JavaClassLibrary"/>
		<rdfs:comment xml:lang="en">JavaLibrary implementing the javax.swing.event package for J2SE 1.2</rdfs:comment>
		<rdfs:comment xml:lang="OWLManchester">platform:implementsInterface some JavaxSwingEventAPI</rdfs:comment>
	</owl:Class>
	<owl:Class rdf:about="&j2se-1_2;JavaxSwingTextClassLibrary">
		<rdfs:subClassOf rdf:resource="&java;JavaClassLibrary"/>
		<rdfs:comment xml:lang="en">JavaLibrary implementing the javax.swing.text package for J2SE 1.2</rdfs:comment>
		<rdfs:comment xml:lang="OWLManchester">platform:implementsInterface some JavaxSwingTextAPI</rdfs:comment>
	</owl:Class>
	<owl:Class rdf:about="&j2se-1_2;JavaxSwingTextHtmlClassLibrary">
		<rdfs:subClassOf rdf:resource="&java;JavaClassLibrary"/>
		<rdfs:comment xml:lang="en">JavaLibrary implementing the javax.swing.text.html package for J2SE 1.2</rdfs:comment>
		<rdfs:comment xml:lang="OWLManchester">platform:implementsInterface some JavaxSwingTextHtmlAPI</rdfs:comment>
	</owl:Class>
	<owl:Class rdf:about="&j2se-1_2;JavaxSwingTextHtmlParserClassLibrary">
		<rdfs:subClassOf rdf:resource="&java;JavaClassLibrary"/>
		<rdfs:comment xml:lang="en">JavaLibrary implementing the javax.swing.text.html.parser package for J2SE 1.2</rdfs:comment>
		<rdfs:comment xml:lang="OWLManchester">platform:implementsInterface some JavaxSwingTextHtmlParserAPI</rdfs:comment>
	</owl:Class>
	<owl:Class rdf:about="&j2se-1_2;JavaxSwingTextRtfClassLibrary">
		<rdfs:subClassOf rdf:resource="&java;JavaClassLibrary"/>
		<rdfs:comment xml:lang="en">JavaLibrary implementing the javax.swing.text.rtf package for J2SE 1.2</rdfs:comment>
		<rdfs:comment xml:lang="OWLManchester">platform:implementsInterface some JavaxSwingTextRtfAPI</rdfs:comment>
	</owl:Class>
	<owl:Class rdf:about="&j2se-1_2;JavaxSwingUndoClassLibrary">
		<rdfs:subClassOf rdf:resource="&java;JavaClassLibrary"/>
		<rdfs:comment xml:lang="en">JavaLibrary implementing the javax.swing.undo package for J2SE 1.2</rdfs:comment>
		<rdfs:comment xml:lang="OWLManchester">platform:implementsInterface some JavaxSwingUndoAPI</rdfs:comment>
	</owl:Class>
	<owl:Class rdf:about="&j2se-1_2;JavaxSwingTableClassLibrary">
		<rdfs:subClassOf rdf:resource="&java;JavaClassLibrary"/>
		<rdfs:comment xml:lang="en">JavaLibrary implementing the javax.swing.table package for J2SE 1.2</rdfs:comment>
		<rdfs:comment xml:lang="OWLManchester">platform:implementsInterface some JavaxSwingTableAPI</rdfs:comment>
	</owl:Class>
	<owl:Class rdf:about="&j2se-1_2;JavaxSwingTreeClassLibrary">
		<rdfs:subClassOf rdf:resource="&java;JavaClassLibrary"/>
		<rdfs:comment xml:lang="en">JavaLibrary implementing the javax.swing.tree package for J2SE 1.2</rdfs:comment>
		<rdfs:comment xml:lang="OWLManchester">platform:implementsInterface some JavaxSwingTreeAPI</rdfs:comment>
	</owl:Class>
	<owl:Class rdf:about="&j2se-1_2;JavaxSwingPlafClassLibrary">
		<rdfs:subClassOf rdf:resource="&java;JavaClassLibrary"/>
		<rdfs:comment xml:lang="en">JavaLibrary implementing the javax.swing.plaf package for J2SE 1.2</rdfs:comment>
		<rdfs:comment xml:lang="OWLManchester">platform:implementsInterface some JavaxSwingPlafAPI</rdfs:comment>
	</owl:Class>
	<owl:Class rdf:about="&j2se-1_2;JavaxSwingPlafBasicClassLibrary">
		<rdfs:subClassOf rdf:resource="&java;JavaClassLibrary"/>
		<rdfs:comment xml:lang="en">JavaLibrary implementing the javax.swing.plaf.basic package for J2SE 1.2</rdfs:comment>
		<rdfs:comment xml:lang="OWLManchester">platform:implementsInterface some JavaxSwingPlafBasicAPI</rdfs:comment>
	</owl:Class>
	<owl:Class rdf:about="&j2se-1_2;JavaxSwingPlafMetalClassLibrary">
		<rdfs:subClassOf rdf:resource="&java;JavaClassLibrary"/>
		<rdfs:comment xml:lang="en">JavaLibrary implementing the javax.swing.plaf.metal package for J2SE 1.2</rdfs:comment>
		<rdfs:comment xml:lang="OWLManchester">platform:implementsInterface some JavaxSwingPlafMetalAPI</rdfs:comment>
	</owl:Class>
	<owl:Class rdf:about="&j2se-1_2;JavaxSwingPlafMultiClassLibrary">
		<rdfs:subClassOf rdf:resource="&java;JavaClassLibrary"/>
		<rdfs:comment xml:lang="en">JavaLibrary implementing the javax.swing.plaf.multi package for J2SE 1.2</rdfs:comment>
		<rdfs:comment xml:lang="OWLManchester">platform:implementsInterface some JavaxSwingPlafMultiAPI</rdfs:comment>
	</owl:Class>
	<owl:Class rdf:about="&j2se-1_2;JavaxSwingBorderClassLibrary">
		<rdfs:subClassOf rdf:resource="&java;JavaClassLibrary"/>
		<rdfs:comment xml:lang="en">JavaLibrary implementing the javax.swing.border package for J2SE 1.2</rdfs:comment>
		<rdfs:comment xml:lang="OWLManchester">platform:implementsInterface some JavaxSwingBorderAPI</rdfs:comment>
	</owl:Class>
	<owl:Class rdf:about="&j2se-1_2;JavaxSwingColorchooserClassLibrary">
		<rdfs:subClassOf rdf:resource="&java;JavaClassLibrary"/>
		<rdfs:comment xml:lang="en">JavaLibrary implementing the javax.swing.colorchooser package for J2SE 1.2</rdfs:comment>
		<rdfs:comment xml:lang="OWLManchester">platform:implementsInterface some JavaxSwingColorchooserAPI</rdfs:comment>
	</owl:Class>
	<owl:Class rdf:about="&j2se-1_2;JavaxSwingFilechooserClassLibrary">
		<rdfs:subClassOf rdf:resource="&java;JavaClassLibrary"/>
		<rdfs:comment xml:lang="en">JavaLibrary implementing the javax.swing.filechooser package for J2SE 1.2</rdfs:comment>
		<rdfs:comment xml:lang="OWLManchester">platform:implementsInterface some JavaxSwingFilechooserAPI</rdfs:comment>
	</owl:Class>
	<owl:Class rdf:about="&j2se-1_2;JavaxAccessibilityClassLibrary">
		<rdfs:subClassOf rdf:resource="&java;JavaClassLibrary"/>
		<rdfs:comment xml:lang="en">JavaLibrary implementing the javax.accessibility package for J2SE 1.2</rdfs:comment>
		<rdfs:comment xml:lang="OWLManchester">platform:implementsInterface some JavaxAccessibilityAPI</rdfs:comment>
	</owl:Class>
	<owl:Class rdf:about="&j2se-1_2;OrgOmgCORBAClassLibrary">
		<rdfs:subClassOf rdf:resource="&java;JavaClassLibrary"/>
		<rdfs:comment xml:lang="en">JavaLibrary implementing the org.omg.CORBA package for J2SE 1.2</rdfs:comment>
		<rdfs:comment xml:lang="OWLManchester">platform:implementsInterface some OrgOmgCORBAAPI</rdfs:comment>
	</owl:Class>
	<owl:Class rdf:about="&j2se-1_2;OrgOmgCORBAPortableClassLibrary">
		<rdfs:subClassOf rdf:resource="&java;JavaClassLibrary"/>
		<rdfs:comment xml:lang="en">JavaLibrary implementing the org.omg.CORBA.portable package for J2SE 1.2</rdfs:comment>
		<rdfs:comment xml:lang="OWLManchester">platform:implementsInterface some OrgOmgCORBAPortableAPI</rdfs:comment>
	</owl:Class>
	<owl:Class rdf:about="&j2se-1_2;OrgOmgCORBADynAnyPackageClassLibrary">
		<rdfs:subClassOf rdf:resource="&java;JavaClassLibrary"/>
		<rdfs:comment xml:lang="en">JavaLibrary implementing the org.omg.CORBA.DynAnyPackage package for J2SE 1.2</rdfs:comment>
		<rdfs:comment xml:lang="OWLManchester">platform:implementsInterface some OrgOmgCORBADynAnyPackageAPI</rdfs:comment>
	</owl:Class>
	<owl:Class rdf:about="&j2se-1_2;OrgOmgCORBAORBPackageClassLibrary">
		<rdfs:subClassOf rdf:resource="&java;JavaClassLibrary"/>
		<rdfs:comment xml:lang="en">JavaLibrary implementing the org.omg.CORBA.ORBPackage package for J2SE 1.2</rdfs:comment>
		<rdfs:comment xml:lang="OWLManchester">platform:implementsInterface some OrgOmgCORBAORBPackageAPI</rdfs:comment>
	</owl:Class>
	<owl:Class rdf:about="&j2se-1_2;OrgOmgCORBATypeCodePackageClassLibrary">
		<rdfs:subClassOf rdf:resource="&java;JavaClassLibrary"/>
		<rdfs:comment xml:lang="en">JavaLibrary implementing the org.omg.CORBA.TypeCodePackage package for J2SE 1.2</rdfs:comment>
		<rdfs:comment xml:lang="OWLManchester">platform:implementsInterface some OrgOmgCORBATypeCodePackageAPI</rdfs:comment>
	</owl:Class>
	<owl:Class rdf:about="&j2se-1_2;OrgOmgCosNamingClassLibrary">
		<rdfs:subClassOf rdf:resource="&java;JavaClassLibrary"/>
		<rdfs:comment xml:lang="en">JavaLibrary implementing the org.omg.CosNaming package for J2SE 1.2</rdfs:comment>
		<rdfs:comment xml:lang="OWLManchester">platform:implementsInterface some OrgOmgCosNamingAPI</rdfs:comment>
	</owl:Class>
	<owl:Class rdf:about="&j2se-1_2;OrgOmgCosNamingNamingContextPackageClassLibrary">
		<rdfs:subClassOf rdf:resource="&java;JavaClassLibrary"/>
		<rdfs:comment xml:lang="en">JavaLibrary implementing the org.omg.CosNaming.NamingContextPackage package for J2SE 1.2</rdfs:comment>
		<rdfs:comment xml:lang="OWLManchester">platform:implementsInterface some OrgOmgCosNamingNamingContextPackageAPI</rdfs:comment>
	</owl:Class>
</rdf:RDF>
