<?xml version="1.0" encoding="ISO-8859-1"?>
<!DOCTYPE rdf:RDF [
	<!ENTITY ns_19 "http://localhost/~dennis/platformkit/2010_1/">
	<!ENTITY j2se-5_0 "http://soft.vub.ac.be/platformkit/2010/1/j2se-5_0.owl#">
	<!ENTITY java-se-6 "http://soft.vub.ac.be/platformkit/2010/1/java-se-6.owl#">
	<!ENTITY isa "http://localhost/~dennis/platformkit/2010_1/isa.owl#">
	<!ENTITY xsd "http://www.w3.org/2001/XMLSchema#">
	<!ENTITY platform "http://localhost/~dennis/platformkit/2010_1/platform.owl#">
	<!ENTITY java "http://localhost/~dennis/platformkit/2010_1/java.owl#">
	<!ENTITY rdf "http://www.w3.org/1999/02/22-rdf-syntax-ns#">
	<!ENTITY rdfs "http://www.w3.org/2000/01/rdf-schema#">
	<!ENTITY owl "http://www.w3.org/2002/07/owl#">
]>
<rdf:RDF
	 xmlns:ns_19="&ns_19;"
	 xmlns:j2se-5_0="&j2se-5_0;"
	 xmlns:java-se-6="&java-se-6;"
	 xmlns:isa="&isa;"
	 xmlns:xsd="&xsd;"
	 xmlns:platform="&platform;"
	 xmlns:java="&java;"
	 xmlns:rdf="&rdf;"
	 xmlns:rdfs="&rdfs;"
	 xmlns:owl="&owl;"
>

	<owl:Ontology rdf:about="http://soft.vub.ac.be/platformkit/2010/1/java-se-6.owl#">
		<owl:versionInfo>$Id: UML2ToPackageAPIOntology.atl 8082 2010-03-18 21:11:00Z dwagelaa $</owl:versionInfo>
		<owl:imports rdf:resource="http://localhost/~dennis/platformkit/2010_1/platform.owl"/>
		<owl:imports rdf:resource="http://localhost/~dennis/platformkit/2010_1/java.owl"/>
		<owl:imports rdf:resource="http://soft.vub.ac.be/platformkit/2010/1/j2se-5_0.owl#"/>
		<owl:imports rdf:resource="http://localhost/~dennis/platformkit/2010_1/isa.owl"/>
		<rdfs:comment xml:lang="en">Generated by [UML2ToSimplifiedPackageAPIOntology.atl 8080 2010-03-18 10:46:40Z dwagelaa], [UML2ToPackageAPIOntology.atl 8082 2010-03-18 21:11:00Z dwagelaa], [UML2ToAPIOntology.atl 8082 2010-03-18 21:11:00Z dwagelaa], and [UML2Comparison.atl 8082 2010-03-18 21:11:00Z dwagelaa]</rdfs:comment>
		<rdfs:comment>Dennis Wagelaar &lt;dennis.wagelaar@vub.ac.be&gt;</rdfs:comment>
		<rdfs:comment xml:lang="en">&#169; 2010, Vrije Universiteit Brussel. All rights reserved.</rdfs:comment>
		<rdfs:label xml:lang="en">Java SE 6</rdfs:label>
	</owl:Ontology>
	<owl:Class rdf:about="&java-se-6;JavaSE6API">
		<rdfs:subClassOf rdf:resource="&java-se-6;JavaxJnlpAPI"/>
		<rdfs:subClassOf rdf:resource="&java-se-6;JavaxCryptoAPI"/>
		<rdfs:subClassOf rdf:resource="&java-se-6;JavaxCryptoInterfacesAPI"/>
		<rdfs:subClassOf rdf:resource="&java-se-6;JavaxCryptoSpecAPI"/>
		<rdfs:subClassOf rdf:resource="&java-se-6;JavaxNetAPI"/>
		<rdfs:subClassOf rdf:resource="&java-se-6;JavaxNetSslAPI"/>
		<rdfs:subClassOf rdf:resource="&java-se-6;JavaxSecurityCertAPI"/>
		<rdfs:subClassOf rdf:resource="&java-se-6;JavaxSecurityAuthAPI"/>
		<rdfs:subClassOf rdf:resource="&java-se-6;JavaxSecurityAuthCallbackAPI"/>
		<rdfs:subClassOf rdf:resource="&java-se-6;JavaxSecurityAuthLoginAPI"/>
		<rdfs:subClassOf rdf:resource="&java-se-6;JavaxSecurityAuthX500API"/>
		<rdfs:subClassOf rdf:resource="&java-se-6;JavaxSecurityAuthKerberosAPI"/>
		<rdfs:subClassOf rdf:resource="&java-se-6;JavaxSecurityAuthSpiAPI"/>
		<rdfs:subClassOf rdf:resource="&java-se-6;JavaxSecuritySaslAPI"/>
		<rdfs:subClassOf rdf:resource="&java-se-6;JavaxAccessibilityAPI"/>
		<rdfs:subClassOf rdf:resource="&java-se-6;JavaxSwingAPI"/>
		<rdfs:subClassOf rdf:resource="&java-se-6;JavaxSwingTextAPI"/>
		<rdfs:subClassOf rdf:resource="&java-se-6;JavaxSwingTextHtmlAPI"/>
		<rdfs:subClassOf rdf:resource="&java-se-6;JavaxSwingTextHtmlParserAPI"/>
		<rdfs:subClassOf rdf:resource="&java-se-6;JavaxSwingTextRtfAPI"/>
		<rdfs:subClassOf rdf:resource="&java-se-6;JavaxSwingEventAPI"/>
		<rdfs:subClassOf rdf:resource="&java-se-6;JavaxSwingColorchooserAPI"/>
		<rdfs:subClassOf rdf:resource="&java-se-6;JavaxSwingPlafAPI"/>
		<rdfs:subClassOf rdf:resource="&java-se-6;JavaxSwingPlafBasicAPI"/>
		<rdfs:subClassOf rdf:resource="&java-se-6;JavaxSwingPlafMetalAPI"/>
		<rdfs:subClassOf rdf:resource="&java-se-6;JavaxSwingPlafMultiAPI"/>
		<rdfs:subClassOf rdf:resource="&java-se-6;JavaxSwingPlafSynthAPI"/>
		<rdfs:subClassOf rdf:resource="&java-se-6;JavaxSwingFilechooserAPI"/>
		<rdfs:subClassOf rdf:resource="&java-se-6;JavaxSwingTreeAPI"/>
		<rdfs:subClassOf rdf:resource="&java-se-6;JavaxSwingBorderAPI"/>
		<rdfs:subClassOf rdf:resource="&java-se-6;JavaxSwingTableAPI"/>
		<rdfs:subClassOf rdf:resource="&java-se-6;JavaxSwingUndoAPI"/>
		<rdfs:subClassOf rdf:resource="&java-se-6;JavaxManagementAPI"/>
		<rdfs:subClassOf rdf:resource="&java-se-6;JavaxManagementOpenmbeanAPI"/>
		<rdfs:subClassOf rdf:resource="&java-se-6;JavaxManagementLoadingAPI"/>
		<rdfs:subClassOf rdf:resource="&java-se-6;JavaxManagementModelmbeanAPI"/>
		<rdfs:subClassOf rdf:resource="&java-se-6;JavaxManagementMonitorAPI"/>
		<rdfs:subClassOf rdf:resource="&java-se-6;JavaxManagementRelationAPI"/>
		<rdfs:subClassOf rdf:resource="&java-se-6;JavaxManagementRemoteAPI"/>
		<rdfs:subClassOf rdf:resource="&java-se-6;JavaxManagementRemoteRmiAPI"/>
		<rdfs:subClassOf rdf:resource="&java-se-6;JavaxManagementTimerAPI"/>
		<rdfs:subClassOf rdf:resource="&java-se-6;JavaxXmlAPI"/>
		<rdfs:subClassOf rdf:resource="&java-se-6;JavaxXmlTransformAPI"/>
		<rdfs:subClassOf rdf:resource="&java-se-6;JavaxXmlTransformDomAPI"/>
		<rdfs:subClassOf rdf:resource="&java-se-6;JavaxXmlTransformSaxAPI"/>
		<rdfs:subClassOf rdf:resource="&java-se-6;JavaxXmlTransformStaxAPI"/>
		<rdfs:subClassOf rdf:resource="&java-se-6;JavaxXmlTransformStreamAPI"/>
		<rdfs:subClassOf rdf:resource="&java-se-6;JavaxXmlBindAPI"/>
		<rdfs:subClassOf rdf:resource="&java-se-6;JavaxXmlBindAnnotationAPI"/>
		<rdfs:subClassOf rdf:resource="&java-se-6;JavaxXmlBindAnnotationAdaptersAPI"/>
		<rdfs:subClassOf rdf:resource="&java-se-6;JavaxXmlBindAttachmentAPI"/>
		<rdfs:subClassOf rdf:resource="&java-se-6;JavaxXmlBindHelpersAPI"/>
		<rdfs:subClassOf rdf:resource="&java-se-6;JavaxXmlBindUtilAPI"/>
		<rdfs:subClassOf rdf:resource="&java-se-6;JavaxXmlValidationAPI"/>
		<rdfs:subClassOf rdf:resource="&java-se-6;JavaxXmlNamespaceAPI"/>
		<rdfs:subClassOf rdf:resource="&java-se-6;JavaxXmlStreamAPI"/>
		<rdfs:subClassOf rdf:resource="&java-se-6;JavaxXmlStreamEventsAPI"/>
		<rdfs:subClassOf rdf:resource="&java-se-6;JavaxXmlStreamUtilAPI"/>
		<rdfs:subClassOf rdf:resource="&java-se-6;JavaxXmlParsersAPI"/>
		<rdfs:subClassOf rdf:resource="&java-se-6;JavaxXmlCryptoAPI"/>
		<rdfs:subClassOf rdf:resource="&java-se-6;JavaxXmlCryptoDsigAPI"/>
		<rdfs:subClassOf rdf:resource="&java-se-6;JavaxXmlCryptoDsigKeyinfoAPI"/>
		<rdfs:subClassOf rdf:resource="&java-se-6;JavaxXmlCryptoDsigSpecAPI"/>
		<rdfs:subClassOf rdf:resource="&java-se-6;JavaxXmlCryptoDsigDomAPI"/>
		<rdfs:subClassOf rdf:resource="&java-se-6;JavaxXmlCryptoDomAPI"/>
		<rdfs:subClassOf rdf:resource="&java-se-6;JavaxXmlDatatypeAPI"/>
		<rdfs:subClassOf rdf:resource="&java-se-6;JavaxXmlSoapAPI"/>
		<rdfs:subClassOf rdf:resource="&java-se-6;JavaxXmlWsAPI"/>
		<rdfs:subClassOf rdf:resource="&java-se-6;JavaxXmlWsHandlerAPI"/>
		<rdfs:subClassOf rdf:resource="&java-se-6;JavaxXmlWsHandlerSoapAPI"/>
		<rdfs:subClassOf rdf:resource="&java-se-6;JavaxXmlWsHttpAPI"/>
		<rdfs:subClassOf rdf:resource="&java-se-6;JavaxXmlWsSoapAPI"/>
		<rdfs:subClassOf rdf:resource="&java-se-6;JavaxXmlWsSpiAPI"/>
		<rdfs:subClassOf rdf:resource="&java-se-6;JavaxXmlWsWsaddressingAPI"/>
		<rdfs:subClassOf rdf:resource="&java-se-6;JavaxXmlXpathAPI"/>
		<rdfs:subClassOf rdf:resource="&java-se-6;JavaxActivationAPI"/>
		<rdfs:subClassOf rdf:resource="&java-se-6;JavaxActivityAPI"/>
		<rdfs:subClassOf rdf:resource="&java-se-6;JavaxAnnotationAPI"/>
		<rdfs:subClassOf rdf:resource="&java-se-6;JavaxAnnotationProcessingAPI"/>
		<rdfs:subClassOf rdf:resource="&java-se-6;JavaxLangModelAPI"/>
		<rdfs:subClassOf rdf:resource="&java-se-6;JavaxLangModelElementAPI"/>
		<rdfs:subClassOf rdf:resource="&java-se-6;JavaxLangModelUtilAPI"/>
		<rdfs:subClassOf rdf:resource="&java-se-6;JavaxLangModelTypeAPI"/>
		<rdfs:subClassOf rdf:resource="&java-se-6;JavaxToolsAPI"/>
		<rdfs:subClassOf rdf:resource="&java-se-6;JavaxImageioAPI"/>
		<rdfs:subClassOf rdf:resource="&java-se-6;JavaxImageioMetadataAPI"/>
		<rdfs:subClassOf rdf:resource="&java-se-6;JavaxImageioStreamAPI"/>
		<rdfs:subClassOf rdf:resource="&java-se-6;JavaxImageioSpiAPI"/>
		<rdfs:subClassOf rdf:resource="&java-se-6;JavaxImageioEventAPI"/>
		<rdfs:subClassOf rdf:resource="&java-se-6;JavaxImageioPluginsBmpAPI"/>
		<rdfs:subClassOf rdf:resource="&java-se-6;JavaxImageioPluginsJpegAPI"/>
		<rdfs:subClassOf rdf:resource="&java-se-6;JavaxJwsAPI"/>
		<rdfs:subClassOf rdf:resource="&java-se-6;JavaxJwsSoapAPI"/>
		<rdfs:subClassOf rdf:resource="&java-se-6;JavaxRmiAPI"/>
		<rdfs:subClassOf rdf:resource="&java-se-6;JavaxRmiCORBAAPI"/>
		<rdfs:subClassOf rdf:resource="&java-se-6;JavaxRmiSslAPI"/>
		<rdfs:subClassOf rdf:resource="&java-se-6;JavaxNamingAPI"/>
		<rdfs:subClassOf rdf:resource="&java-se-6;JavaxNamingDirectoryAPI"/>
		<rdfs:subClassOf rdf:resource="&java-se-6;JavaxNamingEventAPI"/>
		<rdfs:subClassOf rdf:resource="&java-se-6;JavaxNamingLdapAPI"/>
		<rdfs:subClassOf rdf:resource="&java-se-6;JavaxNamingSpiAPI"/>
		<rdfs:subClassOf rdf:resource="&java-se-6;JavaxPrintAPI"/>
		<rdfs:subClassOf rdf:resource="&java-se-6;JavaxPrintAttributeAPI"/>
		<rdfs:subClassOf rdf:resource="&java-se-6;JavaxPrintAttributeStandardAPI"/>
		<rdfs:subClassOf rdf:resource="&java-se-6;JavaxPrintEventAPI"/>
		<rdfs:subClassOf rdf:resource="&java-se-6;JavaxScriptAPI"/>
		<rdfs:subClassOf rdf:resource="&java-se-6;JavaxSmartcardioAPI"/>
		<rdfs:subClassOf rdf:resource="&java-se-6;JavaxSoundMidiAPI"/>
		<rdfs:subClassOf rdf:resource="&java-se-6;JavaxSoundMidiSpiAPI"/>
		<rdfs:subClassOf rdf:resource="&java-se-6;JavaxSoundSampledAPI"/>
		<rdfs:subClassOf rdf:resource="&java-se-6;JavaxSoundSampledSpiAPI"/>
		<rdfs:subClassOf rdf:resource="&java-se-6;JavaxSqlAPI"/>
		<rdfs:subClassOf rdf:resource="&java-se-6;JavaxSqlRowsetAPI"/>
		<rdfs:subClassOf rdf:resource="&java-se-6;JavaxSqlRowsetSpiAPI"/>
		<rdfs:subClassOf rdf:resource="&java-se-6;JavaxSqlRowsetSerialAPI"/>
		<rdfs:subClassOf rdf:resource="&java-se-6;JavaxTransactionAPI"/>
		<rdfs:subClassOf rdf:resource="&java-se-6;JavaxTransactionXaAPI"/>
		<rdfs:subClassOf rdf:resource="&java-se-6;JavaLangAPI"/>
		<rdfs:subClassOf rdf:resource="&java-se-6;JavaLangAnnotationAPI"/>
		<rdfs:subClassOf rdf:resource="&java-se-6;JavaLangReflectAPI"/>
		<rdfs:subClassOf rdf:resource="&java-se-6;JavaLangInstrumentAPI"/>
		<rdfs:subClassOf rdf:resource="&java-se-6;JavaLangManagementAPI"/>
		<rdfs:subClassOf rdf:resource="&java-se-6;JavaLangRefAPI"/>
		<rdfs:subClassOf rdf:resource="&java-se-6;JavaAwtAPI"/>
		<rdfs:subClassOf rdf:resource="&java-se-6;JavaAwtPrintAPI"/>
		<rdfs:subClassOf rdf:resource="&java-se-6;JavaAwtDatatransferAPI"/>
		<rdfs:subClassOf rdf:resource="&java-se-6;JavaAwtEventAPI"/>
		<rdfs:subClassOf rdf:resource="&java-se-6;JavaAwtImageAPI"/>
		<rdfs:subClassOf rdf:resource="&java-se-6;JavaAwtImageRenderableAPI"/>
		<rdfs:subClassOf rdf:resource="&java-se-6;JavaAwtGeomAPI"/>
		<rdfs:subClassOf rdf:resource="&java-se-6;JavaAwtImAPI"/>
		<rdfs:subClassOf rdf:resource="&java-se-6;JavaAwtImSpiAPI"/>
		<rdfs:subClassOf rdf:resource="&java-se-6;JavaAwtColorAPI"/>
		<rdfs:subClassOf rdf:resource="&java-se-6;JavaAwtDndAPI"/>
		<rdfs:subClassOf rdf:resource="&java-se-6;JavaAwtFontAPI"/>
		<rdfs:subClassOf rdf:resource="&java-se-6;JavaNetAPI"/>
		<rdfs:subClassOf rdf:resource="&java-se-6;JavaIoAPI"/>
		<rdfs:subClassOf rdf:resource="&java-se-6;JavaSecurityAPI"/>
		<rdfs:subClassOf rdf:resource="&java-se-6;JavaSecuritySpecAPI"/>
		<rdfs:subClassOf rdf:resource="&java-se-6;JavaSecurityCertAPI"/>
		<rdfs:subClassOf rdf:resource="&java-se-6;JavaSecurityAclAPI"/>
		<rdfs:subClassOf rdf:resource="&java-se-6;JavaSecurityInterfacesAPI"/>
		<rdfs:subClassOf rdf:resource="&java-se-6;JavaMathAPI"/>
		<rdfs:subClassOf rdf:resource="&java-se-6;JavaNioAPI"/>
		<rdfs:subClassOf rdf:resource="&java-se-6;JavaNioChannelsAPI"/>
		<rdfs:subClassOf rdf:resource="&java-se-6;JavaNioChannelsSpiAPI"/>
		<rdfs:subClassOf rdf:resource="&java-se-6;JavaNioCharsetAPI"/>
		<rdfs:subClassOf rdf:resource="&java-se-6;JavaNioCharsetSpiAPI"/>
		<rdfs:subClassOf rdf:resource="&java-se-6;JavaUtilAPI"/>
		<rdfs:subClassOf rdf:resource="&java-se-6;JavaUtilJarAPI"/>
		<rdfs:subClassOf rdf:resource="&java-se-6;JavaUtilSpiAPI"/>
		<rdfs:subClassOf rdf:resource="&java-se-6;JavaUtilConcurrentAPI"/>
		<rdfs:subClassOf rdf:resource="&java-se-6;JavaUtilConcurrentAtomicAPI"/>
		<rdfs:subClassOf rdf:resource="&java-se-6;JavaUtilConcurrentLocksAPI"/>
		<rdfs:subClassOf rdf:resource="&java-se-6;JavaUtilZipAPI"/>
		<rdfs:subClassOf rdf:resource="&java-se-6;JavaUtilLoggingAPI"/>
		<rdfs:subClassOf rdf:resource="&java-se-6;JavaUtilPrefsAPI"/>
		<rdfs:subClassOf rdf:resource="&java-se-6;JavaUtilRegexAPI"/>
		<rdfs:subClassOf rdf:resource="&java-se-6;JavaAppletAPI"/>
		<rdfs:subClassOf rdf:resource="&java-se-6;JavaBeansAPI"/>
		<rdfs:subClassOf rdf:resource="&java-se-6;JavaBeansBeancontextAPI"/>
		<rdfs:subClassOf rdf:resource="&java-se-6;JavaTextAPI"/>
		<rdfs:subClassOf rdf:resource="&java-se-6;JavaTextSpiAPI"/>
		<rdfs:subClassOf rdf:resource="&java-se-6;JavaRmiAPI"/>
		<rdfs:subClassOf rdf:resource="&java-se-6;JavaRmiActivationAPI"/>
		<rdfs:subClassOf rdf:resource="&java-se-6;JavaRmiServerAPI"/>
		<rdfs:subClassOf rdf:resource="&java-se-6;JavaRmiDgcAPI"/>
		<rdfs:subClassOf rdf:resource="&java-se-6;JavaRmiRegistryAPI"/>
		<rdfs:subClassOf rdf:resource="&java-se-6;JavaSqlAPI"/>
		<rdfs:subClassOf rdf:resource="&java-se-6;OrgW3cDomAPI"/>
		<rdfs:subClassOf rdf:resource="&java-se-6;OrgW3cDomLsAPI"/>
		<rdfs:subClassOf rdf:resource="&java-se-6;OrgW3cDomBootstrapAPI"/>
		<rdfs:subClassOf rdf:resource="&java-se-6;OrgW3cDomCssAPI"/>
		<rdfs:subClassOf rdf:resource="&java-se-6;OrgW3cDomStylesheetsAPI"/>
		<rdfs:subClassOf rdf:resource="&java-se-6;OrgW3cDomViewsAPI"/>
		<rdfs:subClassOf rdf:resource="&java-se-6;OrgW3cDomEventsAPI"/>
		<rdfs:subClassOf rdf:resource="&java-se-6;OrgW3cDomHtmlAPI"/>
		<rdfs:subClassOf rdf:resource="&java-se-6;OrgW3cDomTraversalAPI"/>
		<rdfs:subClassOf rdf:resource="&java-se-6;OrgW3cDomRangesAPI"/>
		<rdfs:subClassOf rdf:resource="&java-se-6;OrgW3cDomXpathAPI"/>
		<rdfs:subClassOf rdf:resource="&java-se-6;OrgOmgCORBA_2_3API"/>
		<rdfs:subClassOf rdf:resource="&java-se-6;OrgOmgCORBA_2_3PortableAPI"/>
		<rdfs:subClassOf rdf:resource="&java-se-6;OrgOmgCORBAAPI"/>
		<rdfs:subClassOf rdf:resource="&java-se-6;OrgOmgCORBAPortableAPI"/>
		<rdfs:subClassOf rdf:resource="&java-se-6;OrgOmgCORBADynAnyPackageAPI"/>
		<rdfs:subClassOf rdf:resource="&java-se-6;OrgOmgCORBAORBPackageAPI"/>
		<rdfs:subClassOf rdf:resource="&java-se-6;OrgOmgCORBATypeCodePackageAPI"/>
		<rdfs:subClassOf rdf:resource="&java-se-6;OrgOmgSendingContextAPI"/>
		<rdfs:subClassOf rdf:resource="&java-se-6;OrgOmgCosNamingAPI"/>
		<rdfs:subClassOf rdf:resource="&java-se-6;OrgOmgCosNamingNamingContextExtPackageAPI"/>
		<rdfs:subClassOf rdf:resource="&java-se-6;OrgOmgCosNamingNamingContextPackageAPI"/>
		<rdfs:subClassOf rdf:resource="&java-se-6;OrgOmgPortableServerAPI"/>
		<rdfs:subClassOf rdf:resource="&java-se-6;OrgOmgPortableServerCurrentPackageAPI"/>
		<rdfs:subClassOf rdf:resource="&java-se-6;OrgOmgPortableServerPOAManagerPackageAPI"/>
		<rdfs:subClassOf rdf:resource="&java-se-6;OrgOmgPortableServerPOAPackageAPI"/>
		<rdfs:subClassOf rdf:resource="&java-se-6;OrgOmgPortableServerPortableAPI"/>
		<rdfs:subClassOf rdf:resource="&java-se-6;OrgOmgPortableServerServantLocatorPackageAPI"/>
		<rdfs:subClassOf rdf:resource="&java-se-6;OrgOmgDynamicAPI"/>
		<rdfs:subClassOf rdf:resource="&java-se-6;OrgOmgDynamicAnyAPI"/>
		<rdfs:subClassOf rdf:resource="&java-se-6;OrgOmgDynamicAnyDynAnyFactoryPackageAPI"/>
		<rdfs:subClassOf rdf:resource="&java-se-6;OrgOmgDynamicAnyDynAnyPackageAPI"/>
		<rdfs:subClassOf rdf:resource="&java-se-6;OrgOmgIOPAPI"/>
		<rdfs:subClassOf rdf:resource="&java-se-6;OrgOmgIOPCodecFactoryPackageAPI"/>
		<rdfs:subClassOf rdf:resource="&java-se-6;OrgOmgIOPCodecPackageAPI"/>
		<rdfs:subClassOf rdf:resource="&java-se-6;OrgOmgMessagingAPI"/>
		<rdfs:subClassOf rdf:resource="&java-se-6;OrgOmgPortableInterceptorAPI"/>
		<rdfs:subClassOf rdf:resource="&java-se-6;OrgOmgPortableInterceptorORBInitInfoPackageAPI"/>
		<rdfs:subClassOf rdf:resource="&java-se-6;OrgOmgStubJavaRmiAPI"/>
		<rdfs:subClassOf rdf:resource="&java-se-6;OrgOmgStubJavaxManagementRemoteRmiAPI"/>
		<rdfs:subClassOf rdf:resource="&java-se-6;OrgXmlSaxAPI"/>
		<rdfs:subClassOf rdf:resource="&java-se-6;OrgXmlSaxHelpersAPI"/>
		<rdfs:subClassOf rdf:resource="&java-se-6;OrgXmlSaxExtAPI"/>
		<rdfs:subClassOf rdf:resource="&java-se-6;OrgIetfJgssAPI"/>
		<rdfs:comment xml:lang="en">Java SE 6 API</rdfs:comment>
		<rdfs:comment xml:lang="OWLManchester">platform:comprisesInterfacePart some JavaxJnlp and platform:comprisesInterfacePart some JavaxCrypto and platform:comprisesInterfacePart some JavaxCryptoInterfaces and platform:comprisesInterfacePart some JavaxCryptoSpec and platform:comprisesInterfacePart some JavaxNet and platform:comprisesInterfacePart some JavaxNetSsl and platform:comprisesInterfacePart some JavaxSecurityCert and platform:comprisesInterfacePart some JavaxSecurityAuth and platform:comprisesInterfacePart some JavaxSecurityAuthCallback and platform:comprisesInterfacePart some JavaxSecurityAuthLogin and platform:comprisesInterfacePart some JavaxSecurityAuthX500 and platform:comprisesInterfacePart some JavaxSecurityAuthKerberos and platform:comprisesInterfacePart some JavaxSecurityAuthSpi and platform:comprisesInterfacePart some JavaxSecuritySasl and platform:comprisesInterfacePart some JavaxAccessibility and platform:comprisesInterfacePart some JavaxSwing and platform:comprisesInterfacePart some JavaxSwingText and platform:comprisesInterfacePart some JavaxSwingTextHtml and platform:comprisesInterfacePart some JavaxSwingTextHtmlParser and platform:comprisesInterfacePart some JavaxSwingTextRtf and platform:comprisesInterfacePart some JavaxSwingEvent and platform:comprisesInterfacePart some JavaxSwingColorchooser and platform:comprisesInterfacePart some JavaxSwingPlaf and platform:comprisesInterfacePart some JavaxSwingPlafBasic and platform:comprisesInterfacePart some JavaxSwingPlafMetal and platform:comprisesInterfacePart some JavaxSwingPlafMulti and platform:comprisesInterfacePart some JavaxSwingPlafSynth and platform:comprisesInterfacePart some JavaxSwingFilechooser and platform:comprisesInterfacePart some JavaxSwingTree and platform:comprisesInterfacePart some JavaxSwingBorder and platform:comprisesInterfacePart some JavaxSwingTable and platform:comprisesInterfacePart some JavaxSwingUndo and platform:comprisesInterfacePart some JavaxManagement and platform:comprisesInterfacePart some JavaxManagementOpenmbean and platform:comprisesInterfacePart some JavaxManagementLoading and platform:comprisesInterfacePart some JavaxManagementModelmbean and platform:comprisesInterfacePart some JavaxManagementMonitor and platform:comprisesInterfacePart some JavaxManagementRelation and platform:comprisesInterfacePart some JavaxManagementRemote and platform:comprisesInterfacePart some JavaxManagementRemoteRmi and platform:comprisesInterfacePart some JavaxManagementTimer and platform:comprisesInterfacePart some JavaxXml and platform:comprisesInterfacePart some JavaxXmlTransform and platform:comprisesInterfacePart some JavaxXmlTransformDom and platform:comprisesInterfacePart some JavaxXmlTransformSax and platform:comprisesInterfacePart some JavaxXmlTransformStax and platform:comprisesInterfacePart some JavaxXmlTransformStream and platform:comprisesInterfacePart some JavaxXmlBind and platform:comprisesInterfacePart some JavaxXmlBindAnnotation and platform:comprisesInterfacePart some JavaxXmlBindAnnotationAdapters and platform:comprisesInterfacePart some JavaxXmlBindAttachment and platform:comprisesInterfacePart some JavaxXmlBindHelpers and platform:comprisesInterfacePart some JavaxXmlBindUtil and platform:comprisesInterfacePart some JavaxXmlValidation and platform:comprisesInterfacePart some JavaxXmlNamespace and platform:comprisesInterfacePart some JavaxXmlStream and platform:comprisesInterfacePart some JavaxXmlStreamEvents and platform:comprisesInterfacePart some JavaxXmlStreamUtil and platform:comprisesInterfacePart some JavaxXmlParsers and platform:comprisesInterfacePart some JavaxXmlCrypto and platform:comprisesInterfacePart some JavaxXmlCryptoDsig and platform:comprisesInterfacePart some JavaxXmlCryptoDsigKeyinfo and platform:comprisesInterfacePart some JavaxXmlCryptoDsigSpec and platform:comprisesInterfacePart some JavaxXmlCryptoDsigDom and platform:comprisesInterfacePart some JavaxXmlCryptoDom and platform:comprisesInterfacePart some JavaxXmlDatatype and platform:comprisesInterfacePart some JavaxXmlSoap and platform:comprisesInterfacePart some JavaxXmlWs and platform:comprisesInterfacePart some JavaxXmlWsHandler and platform:comprisesInterfacePart some JavaxXmlWsHandlerSoap and platform:comprisesInterfacePart some JavaxXmlWsHttp and platform:comprisesInterfacePart some JavaxXmlWsSoap and platform:comprisesInterfacePart some JavaxXmlWsSpi and platform:comprisesInterfacePart some JavaxXmlWsWsaddressing and platform:comprisesInterfacePart some JavaxXmlXpath and platform:comprisesInterfacePart some JavaxActivation and platform:comprisesInterfacePart some JavaxActivity and platform:comprisesInterfacePart some JavaxAnnotation and platform:comprisesInterfacePart some JavaxAnnotationProcessing and platform:comprisesInterfacePart some JavaxLangModel and platform:comprisesInterfacePart some JavaxLangModelElement and platform:comprisesInterfacePart some JavaxLangModelUtil and platform:comprisesInterfacePart some JavaxLangModelType and platform:comprisesInterfacePart some JavaxTools and platform:comprisesInterfacePart some JavaxImageio and platform:comprisesInterfacePart some JavaxImageioMetadata and platform:comprisesInterfacePart some JavaxImageioStream and platform:comprisesInterfacePart some JavaxImageioSpi and platform:comprisesInterfacePart some JavaxImageioEvent and platform:comprisesInterfacePart some JavaxImageioPluginsBmp and platform:comprisesInterfacePart some JavaxImageioPluginsJpeg and platform:comprisesInterfacePart some JavaxJws and platform:comprisesInterfacePart some JavaxJwsSoap and platform:comprisesInterfacePart some JavaxRmi and platform:comprisesInterfacePart some JavaxRmiCORBA and platform:comprisesInterfacePart some JavaxRmiSsl and platform:comprisesInterfacePart some JavaxNaming and platform:comprisesInterfacePart some JavaxNamingDirectory and platform:comprisesInterfacePart some JavaxNamingEvent and platform:comprisesInterfacePart some JavaxNamingLdap and platform:comprisesInterfacePart some JavaxNamingSpi and platform:comprisesInterfacePart some JavaxPrint and platform:comprisesInterfacePart some JavaxPrintAttribute and platform:comprisesInterfacePart some JavaxPrintAttributeStandard and platform:comprisesInterfacePart some JavaxPrintEvent and platform:comprisesInterfacePart some JavaxScript and platform:comprisesInterfacePart some JavaxSmartcardio and platform:comprisesInterfacePart some JavaxSoundMidi and platform:comprisesInterfacePart some JavaxSoundMidiSpi and platform:comprisesInterfacePart some JavaxSoundSampled and platform:comprisesInterfacePart some JavaxSoundSampledSpi and platform:comprisesInterfacePart some JavaxSql and platform:comprisesInterfacePart some JavaxSqlRowset and platform:comprisesInterfacePart some JavaxSqlRowsetSpi and platform:comprisesInterfacePart some JavaxSqlRowsetSerial and platform:comprisesInterfacePart some JavaxTransaction and platform:comprisesInterfacePart some JavaxTransactionXa and platform:comprisesInterfacePart some JavaLang and platform:comprisesInterfacePart some JavaLangAnnotation and platform:comprisesInterfacePart some JavaLangReflect and platform:comprisesInterfacePart some JavaLangInstrument and platform:comprisesInterfacePart some JavaLangManagement and platform:comprisesInterfacePart some JavaLangRef and platform:comprisesInterfacePart some JavaAwt and platform:comprisesInterfacePart some JavaAwtPrint and platform:comprisesInterfacePart some JavaAwtDatatransfer and platform:comprisesInterfacePart some JavaAwtEvent and platform:comprisesInterfacePart some JavaAwtImage and platform:comprisesInterfacePart some JavaAwtImageRenderable and platform:comprisesInterfacePart some JavaAwtGeom and platform:comprisesInterfacePart some JavaAwtIm and platform:comprisesInterfacePart some JavaAwtImSpi and platform:comprisesInterfacePart some JavaAwtColor and platform:comprisesInterfacePart some JavaAwtDnd and platform:comprisesInterfacePart some JavaAwtFont and platform:comprisesInterfacePart some JavaNet and platform:comprisesInterfacePart some JavaIo and platform:comprisesInterfacePart some JavaSecurity and platform:comprisesInterfacePart some JavaSecuritySpec and platform:comprisesInterfacePart some JavaSecurityCert and platform:comprisesInterfacePart some JavaSecurityAcl and platform:comprisesInterfacePart some JavaSecurityInterfaces and platform:comprisesInterfacePart some JavaMath and platform:comprisesInterfacePart some JavaNio and platform:comprisesInterfacePart some JavaNioChannels and platform:comprisesInterfacePart some JavaNioChannelsSpi and platform:comprisesInterfacePart some JavaNioCharset and platform:comprisesInterfacePart some JavaNioCharsetSpi and platform:comprisesInterfacePart some JavaUtil and platform:comprisesInterfacePart some JavaUtilJar and platform:comprisesInterfacePart some JavaUtilSpi and platform:comprisesInterfacePart some JavaUtilConcurrent and platform:comprisesInterfacePart some JavaUtilConcurrentAtomic and platform:comprisesInterfacePart some JavaUtilConcurrentLocks and platform:comprisesInterfacePart some JavaUtilZip and platform:comprisesInterfacePart some JavaUtilLogging and platform:comprisesInterfacePart some JavaUtilPrefs and platform:comprisesInterfacePart some JavaUtilRegex and platform:comprisesInterfacePart some JavaApplet and platform:comprisesInterfacePart some JavaBeans and platform:comprisesInterfacePart some JavaBeansBeancontext and platform:comprisesInterfacePart some JavaText and platform:comprisesInterfacePart some JavaTextSpi and platform:comprisesInterfacePart some JavaRmi and platform:comprisesInterfacePart some JavaRmiActivation and platform:comprisesInterfacePart some JavaRmiServer and platform:comprisesInterfacePart some JavaRmiDgc and platform:comprisesInterfacePart some JavaRmiRegistry and platform:comprisesInterfacePart some JavaSql and platform:comprisesInterfacePart some OrgW3cDom and platform:comprisesInterfacePart some OrgW3cDomLs and platform:comprisesInterfacePart some OrgW3cDomBootstrap and platform:comprisesInterfacePart some OrgW3cDomCss and platform:comprisesInterfacePart some OrgW3cDomStylesheets and platform:comprisesInterfacePart some OrgW3cDomViews and platform:comprisesInterfacePart some OrgW3cDomEvents and platform:comprisesInterfacePart some OrgW3cDomHtml and platform:comprisesInterfacePart some OrgW3cDomTraversal and platform:comprisesInterfacePart some OrgW3cDomRanges and platform:comprisesInterfacePart some OrgW3cDomXpath and platform:comprisesInterfacePart some OrgOmgCORBA_2_3 and platform:comprisesInterfacePart some OrgOmgCORBA_2_3Portable and platform:comprisesInterfacePart some OrgOmgCORBA and platform:comprisesInterfacePart some OrgOmgCORBAPortable and platform:comprisesInterfacePart some OrgOmgCORBADynAnyPackage and platform:comprisesInterfacePart some OrgOmgCORBAORBPackage and platform:comprisesInterfacePart some OrgOmgCORBATypeCodePackage and platform:comprisesInterfacePart some OrgOmgSendingContext and platform:comprisesInterfacePart some OrgOmgCosNaming and platform:comprisesInterfacePart some OrgOmgCosNamingNamingContextExtPackage and platform:comprisesInterfacePart some OrgOmgCosNamingNamingContextPackage and platform:comprisesInterfacePart some OrgOmgPortableServer and platform:comprisesInterfacePart some OrgOmgPortableServerCurrentPackage and platform:comprisesInterfacePart some OrgOmgPortableServerPOAManagerPackage and platform:comprisesInterfacePart some OrgOmgPortableServerPOAPackage and platform:comprisesInterfacePart some OrgOmgPortableServerPortable and platform:comprisesInterfacePart some OrgOmgPortableServerServantLocatorPackage and platform:comprisesInterfacePart some OrgOmgDynamic and platform:comprisesInterfacePart some OrgOmgDynamicAny and platform:comprisesInterfacePart some OrgOmgDynamicAnyDynAnyFactoryPackage and platform:comprisesInterfacePart some OrgOmgDynamicAnyDynAnyPackage and platform:comprisesInterfacePart some OrgOmgIOP and platform:comprisesInterfacePart some OrgOmgIOPCodecFactoryPackage and platform:comprisesInterfacePart some OrgOmgIOPCodecPackage and platform:comprisesInterfacePart some OrgOmgMessaging and platform:comprisesInterfacePart some OrgOmgPortableInterceptor and platform:comprisesInterfacePart some OrgOmgPortableInterceptorORBInitInfoPackage and platform:comprisesInterfacePart some OrgOmgStubJavaRmi and platform:comprisesInterfacePart some OrgOmgStubJavaxManagementRemoteRmi and platform:comprisesInterfacePart some OrgXmlSax and platform:comprisesInterfacePart some OrgXmlSaxHelpers and platform:comprisesInterfacePart some OrgXmlSaxExt and platform:comprisesInterfacePart some OrgIetfJgss</rdfs:comment>
	</owl:Class>
	<owl:Class rdf:about="&java-se-6;JavaSE6ClassLibrary">
		<rdfs:subClassOf rdf:resource="&java-se-6;JavaxJnlpClassLibrary"/>
		<rdfs:subClassOf rdf:resource="&java-se-6;JavaxCryptoClassLibrary"/>
		<rdfs:subClassOf rdf:resource="&java-se-6;JavaxCryptoInterfacesClassLibrary"/>
		<rdfs:subClassOf rdf:resource="&java-se-6;JavaxCryptoSpecClassLibrary"/>
		<rdfs:subClassOf rdf:resource="&java-se-6;JavaxNetClassLibrary"/>
		<rdfs:subClassOf rdf:resource="&java-se-6;JavaxNetSslClassLibrary"/>
		<rdfs:subClassOf rdf:resource="&java-se-6;JavaxSecurityCertClassLibrary"/>
		<rdfs:subClassOf rdf:resource="&java-se-6;JavaxSecurityAuthClassLibrary"/>
		<rdfs:subClassOf rdf:resource="&java-se-6;JavaxSecurityAuthCallbackClassLibrary"/>
		<rdfs:subClassOf rdf:resource="&java-se-6;JavaxSecurityAuthLoginClassLibrary"/>
		<rdfs:subClassOf rdf:resource="&java-se-6;JavaxSecurityAuthX500ClassLibrary"/>
		<rdfs:subClassOf rdf:resource="&java-se-6;JavaxSecurityAuthKerberosClassLibrary"/>
		<rdfs:subClassOf rdf:resource="&java-se-6;JavaxSecurityAuthSpiClassLibrary"/>
		<rdfs:subClassOf rdf:resource="&java-se-6;JavaxSecuritySaslClassLibrary"/>
		<rdfs:subClassOf rdf:resource="&java-se-6;JavaxAccessibilityClassLibrary"/>
		<rdfs:subClassOf rdf:resource="&java-se-6;JavaxSwingClassLibrary"/>
		<rdfs:subClassOf rdf:resource="&java-se-6;JavaxSwingTextClassLibrary"/>
		<rdfs:subClassOf rdf:resource="&java-se-6;JavaxSwingTextHtmlClassLibrary"/>
		<rdfs:subClassOf rdf:resource="&java-se-6;JavaxSwingTextHtmlParserClassLibrary"/>
		<rdfs:subClassOf rdf:resource="&java-se-6;JavaxSwingTextRtfClassLibrary"/>
		<rdfs:subClassOf rdf:resource="&java-se-6;JavaxSwingEventClassLibrary"/>
		<rdfs:subClassOf rdf:resource="&java-se-6;JavaxSwingColorchooserClassLibrary"/>
		<rdfs:subClassOf rdf:resource="&java-se-6;JavaxSwingPlafClassLibrary"/>
		<rdfs:subClassOf rdf:resource="&java-se-6;JavaxSwingPlafBasicClassLibrary"/>
		<rdfs:subClassOf rdf:resource="&java-se-6;JavaxSwingPlafMetalClassLibrary"/>
		<rdfs:subClassOf rdf:resource="&java-se-6;JavaxSwingPlafMultiClassLibrary"/>
		<rdfs:subClassOf rdf:resource="&java-se-6;JavaxSwingPlafSynthClassLibrary"/>
		<rdfs:subClassOf rdf:resource="&java-se-6;JavaxSwingFilechooserClassLibrary"/>
		<rdfs:subClassOf rdf:resource="&java-se-6;JavaxSwingTreeClassLibrary"/>
		<rdfs:subClassOf rdf:resource="&java-se-6;JavaxSwingBorderClassLibrary"/>
		<rdfs:subClassOf rdf:resource="&java-se-6;JavaxSwingTableClassLibrary"/>
		<rdfs:subClassOf rdf:resource="&java-se-6;JavaxSwingUndoClassLibrary"/>
		<rdfs:subClassOf rdf:resource="&java-se-6;JavaxManagementClassLibrary"/>
		<rdfs:subClassOf rdf:resource="&java-se-6;JavaxManagementOpenmbeanClassLibrary"/>
		<rdfs:subClassOf rdf:resource="&java-se-6;JavaxManagementLoadingClassLibrary"/>
		<rdfs:subClassOf rdf:resource="&java-se-6;JavaxManagementModelmbeanClassLibrary"/>
		<rdfs:subClassOf rdf:resource="&java-se-6;JavaxManagementMonitorClassLibrary"/>
		<rdfs:subClassOf rdf:resource="&java-se-6;JavaxManagementRelationClassLibrary"/>
		<rdfs:subClassOf rdf:resource="&java-se-6;JavaxManagementRemoteClassLibrary"/>
		<rdfs:subClassOf rdf:resource="&java-se-6;JavaxManagementRemoteRmiClassLibrary"/>
		<rdfs:subClassOf rdf:resource="&java-se-6;JavaxManagementTimerClassLibrary"/>
		<rdfs:subClassOf rdf:resource="&java-se-6;JavaxXmlClassLibrary"/>
		<rdfs:subClassOf rdf:resource="&java-se-6;JavaxXmlTransformClassLibrary"/>
		<rdfs:subClassOf rdf:resource="&java-se-6;JavaxXmlTransformDomClassLibrary"/>
		<rdfs:subClassOf rdf:resource="&java-se-6;JavaxXmlTransformSaxClassLibrary"/>
		<rdfs:subClassOf rdf:resource="&java-se-6;JavaxXmlTransformStaxClassLibrary"/>
		<rdfs:subClassOf rdf:resource="&java-se-6;JavaxXmlTransformStreamClassLibrary"/>
		<rdfs:subClassOf rdf:resource="&java-se-6;JavaxXmlBindClassLibrary"/>
		<rdfs:subClassOf rdf:resource="&java-se-6;JavaxXmlBindAnnotationClassLibrary"/>
		<rdfs:subClassOf rdf:resource="&java-se-6;JavaxXmlBindAnnotationAdaptersClassLibrary"/>
		<rdfs:subClassOf rdf:resource="&java-se-6;JavaxXmlBindAttachmentClassLibrary"/>
		<rdfs:subClassOf rdf:resource="&java-se-6;JavaxXmlBindHelpersClassLibrary"/>
		<rdfs:subClassOf rdf:resource="&java-se-6;JavaxXmlBindUtilClassLibrary"/>
		<rdfs:subClassOf rdf:resource="&java-se-6;JavaxXmlValidationClassLibrary"/>
		<rdfs:subClassOf rdf:resource="&java-se-6;JavaxXmlNamespaceClassLibrary"/>
		<rdfs:subClassOf rdf:resource="&java-se-6;JavaxXmlStreamClassLibrary"/>
		<rdfs:subClassOf rdf:resource="&java-se-6;JavaxXmlStreamEventsClassLibrary"/>
		<rdfs:subClassOf rdf:resource="&java-se-6;JavaxXmlStreamUtilClassLibrary"/>
		<rdfs:subClassOf rdf:resource="&java-se-6;JavaxXmlParsersClassLibrary"/>
		<rdfs:subClassOf rdf:resource="&java-se-6;JavaxXmlCryptoClassLibrary"/>
		<rdfs:subClassOf rdf:resource="&java-se-6;JavaxXmlCryptoDsigClassLibrary"/>
		<rdfs:subClassOf rdf:resource="&java-se-6;JavaxXmlCryptoDsigKeyinfoClassLibrary"/>
		<rdfs:subClassOf rdf:resource="&java-se-6;JavaxXmlCryptoDsigSpecClassLibrary"/>
		<rdfs:subClassOf rdf:resource="&java-se-6;JavaxXmlCryptoDsigDomClassLibrary"/>
		<rdfs:subClassOf rdf:resource="&java-se-6;JavaxXmlCryptoDomClassLibrary"/>
		<rdfs:subClassOf rdf:resource="&java-se-6;JavaxXmlDatatypeClassLibrary"/>
		<rdfs:subClassOf rdf:resource="&java-se-6;JavaxXmlSoapClassLibrary"/>
		<rdfs:subClassOf rdf:resource="&java-se-6;JavaxXmlWsClassLibrary"/>
		<rdfs:subClassOf rdf:resource="&java-se-6;JavaxXmlWsHandlerClassLibrary"/>
		<rdfs:subClassOf rdf:resource="&java-se-6;JavaxXmlWsHandlerSoapClassLibrary"/>
		<rdfs:subClassOf rdf:resource="&java-se-6;JavaxXmlWsHttpClassLibrary"/>
		<rdfs:subClassOf rdf:resource="&java-se-6;JavaxXmlWsSoapClassLibrary"/>
		<rdfs:subClassOf rdf:resource="&java-se-6;JavaxXmlWsSpiClassLibrary"/>
		<rdfs:subClassOf rdf:resource="&java-se-6;JavaxXmlWsWsaddressingClassLibrary"/>
		<rdfs:subClassOf rdf:resource="&java-se-6;JavaxXmlXpathClassLibrary"/>
		<rdfs:subClassOf rdf:resource="&java-se-6;JavaxActivationClassLibrary"/>
		<rdfs:subClassOf rdf:resource="&java-se-6;JavaxActivityClassLibrary"/>
		<rdfs:subClassOf rdf:resource="&java-se-6;JavaxAnnotationClassLibrary"/>
		<rdfs:subClassOf rdf:resource="&java-se-6;JavaxAnnotationProcessingClassLibrary"/>
		<rdfs:subClassOf rdf:resource="&java-se-6;JavaxLangModelClassLibrary"/>
		<rdfs:subClassOf rdf:resource="&java-se-6;JavaxLangModelElementClassLibrary"/>
		<rdfs:subClassOf rdf:resource="&java-se-6;JavaxLangModelUtilClassLibrary"/>
		<rdfs:subClassOf rdf:resource="&java-se-6;JavaxLangModelTypeClassLibrary"/>
		<rdfs:subClassOf rdf:resource="&java-se-6;JavaxToolsClassLibrary"/>
		<rdfs:subClassOf rdf:resource="&java-se-6;JavaxImageioClassLibrary"/>
		<rdfs:subClassOf rdf:resource="&java-se-6;JavaxImageioMetadataClassLibrary"/>
		<rdfs:subClassOf rdf:resource="&java-se-6;JavaxImageioStreamClassLibrary"/>
		<rdfs:subClassOf rdf:resource="&java-se-6;JavaxImageioSpiClassLibrary"/>
		<rdfs:subClassOf rdf:resource="&java-se-6;JavaxImageioEventClassLibrary"/>
		<rdfs:subClassOf rdf:resource="&java-se-6;JavaxImageioPluginsBmpClassLibrary"/>
		<rdfs:subClassOf rdf:resource="&java-se-6;JavaxImageioPluginsJpegClassLibrary"/>
		<rdfs:subClassOf rdf:resource="&java-se-6;JavaxJwsClassLibrary"/>
		<rdfs:subClassOf rdf:resource="&java-se-6;JavaxJwsSoapClassLibrary"/>
		<rdfs:subClassOf rdf:resource="&java-se-6;JavaxRmiClassLibrary"/>
		<rdfs:subClassOf rdf:resource="&java-se-6;JavaxRmiCORBAClassLibrary"/>
		<rdfs:subClassOf rdf:resource="&java-se-6;JavaxRmiSslClassLibrary"/>
		<rdfs:subClassOf rdf:resource="&java-se-6;JavaxNamingClassLibrary"/>
		<rdfs:subClassOf rdf:resource="&java-se-6;JavaxNamingDirectoryClassLibrary"/>
		<rdfs:subClassOf rdf:resource="&java-se-6;JavaxNamingEventClassLibrary"/>
		<rdfs:subClassOf rdf:resource="&java-se-6;JavaxNamingLdapClassLibrary"/>
		<rdfs:subClassOf rdf:resource="&java-se-6;JavaxNamingSpiClassLibrary"/>
		<rdfs:subClassOf rdf:resource="&java-se-6;JavaxPrintClassLibrary"/>
		<rdfs:subClassOf rdf:resource="&java-se-6;JavaxPrintAttributeClassLibrary"/>
		<rdfs:subClassOf rdf:resource="&java-se-6;JavaxPrintAttributeStandardClassLibrary"/>
		<rdfs:subClassOf rdf:resource="&java-se-6;JavaxPrintEventClassLibrary"/>
		<rdfs:subClassOf rdf:resource="&java-se-6;JavaxScriptClassLibrary"/>
		<rdfs:subClassOf rdf:resource="&java-se-6;JavaxSmartcardioClassLibrary"/>
		<rdfs:subClassOf rdf:resource="&java-se-6;JavaxSoundMidiClassLibrary"/>
		<rdfs:subClassOf rdf:resource="&java-se-6;JavaxSoundMidiSpiClassLibrary"/>
		<rdfs:subClassOf rdf:resource="&java-se-6;JavaxSoundSampledClassLibrary"/>
		<rdfs:subClassOf rdf:resource="&java-se-6;JavaxSoundSampledSpiClassLibrary"/>
		<rdfs:subClassOf rdf:resource="&java-se-6;JavaxSqlClassLibrary"/>
		<rdfs:subClassOf rdf:resource="&java-se-6;JavaxSqlRowsetClassLibrary"/>
		<rdfs:subClassOf rdf:resource="&java-se-6;JavaxSqlRowsetSpiClassLibrary"/>
		<rdfs:subClassOf rdf:resource="&java-se-6;JavaxSqlRowsetSerialClassLibrary"/>
		<rdfs:subClassOf rdf:resource="&java-se-6;JavaxTransactionClassLibrary"/>
		<rdfs:subClassOf rdf:resource="&java-se-6;JavaxTransactionXaClassLibrary"/>
		<rdfs:subClassOf rdf:resource="&java-se-6;JavaLangClassLibrary"/>
		<rdfs:subClassOf rdf:resource="&java-se-6;JavaLangAnnotationClassLibrary"/>
		<rdfs:subClassOf rdf:resource="&java-se-6;JavaLangReflectClassLibrary"/>
		<rdfs:subClassOf rdf:resource="&java-se-6;JavaLangInstrumentClassLibrary"/>
		<rdfs:subClassOf rdf:resource="&java-se-6;JavaLangManagementClassLibrary"/>
		<rdfs:subClassOf rdf:resource="&java-se-6;JavaLangRefClassLibrary"/>
		<rdfs:subClassOf rdf:resource="&java-se-6;JavaAwtClassLibrary"/>
		<rdfs:subClassOf rdf:resource="&java-se-6;JavaAwtPrintClassLibrary"/>
		<rdfs:subClassOf rdf:resource="&java-se-6;JavaAwtDatatransferClassLibrary"/>
		<rdfs:subClassOf rdf:resource="&java-se-6;JavaAwtEventClassLibrary"/>
		<rdfs:subClassOf rdf:resource="&java-se-6;JavaAwtImageClassLibrary"/>
		<rdfs:subClassOf rdf:resource="&java-se-6;JavaAwtImageRenderableClassLibrary"/>
		<rdfs:subClassOf rdf:resource="&java-se-6;JavaAwtGeomClassLibrary"/>
		<rdfs:subClassOf rdf:resource="&java-se-6;JavaAwtImClassLibrary"/>
		<rdfs:subClassOf rdf:resource="&java-se-6;JavaAwtImSpiClassLibrary"/>
		<rdfs:subClassOf rdf:resource="&java-se-6;JavaAwtColorClassLibrary"/>
		<rdfs:subClassOf rdf:resource="&java-se-6;JavaAwtDndClassLibrary"/>
		<rdfs:subClassOf rdf:resource="&java-se-6;JavaAwtFontClassLibrary"/>
		<rdfs:subClassOf rdf:resource="&java-se-6;JavaNetClassLibrary"/>
		<rdfs:subClassOf rdf:resource="&java-se-6;JavaIoClassLibrary"/>
		<rdfs:subClassOf rdf:resource="&java-se-6;JavaSecurityClassLibrary"/>
		<rdfs:subClassOf rdf:resource="&java-se-6;JavaSecuritySpecClassLibrary"/>
		<rdfs:subClassOf rdf:resource="&java-se-6;JavaSecurityCertClassLibrary"/>
		<rdfs:subClassOf rdf:resource="&java-se-6;JavaSecurityAclClassLibrary"/>
		<rdfs:subClassOf rdf:resource="&java-se-6;JavaSecurityInterfacesClassLibrary"/>
		<rdfs:subClassOf rdf:resource="&java-se-6;JavaMathClassLibrary"/>
		<rdfs:subClassOf rdf:resource="&java-se-6;JavaNioClassLibrary"/>
		<rdfs:subClassOf rdf:resource="&java-se-6;JavaNioChannelsClassLibrary"/>
		<rdfs:subClassOf rdf:resource="&java-se-6;JavaNioChannelsSpiClassLibrary"/>
		<rdfs:subClassOf rdf:resource="&java-se-6;JavaNioCharsetClassLibrary"/>
		<rdfs:subClassOf rdf:resource="&java-se-6;JavaNioCharsetSpiClassLibrary"/>
		<rdfs:subClassOf rdf:resource="&java-se-6;JavaUtilClassLibrary"/>
		<rdfs:subClassOf rdf:resource="&java-se-6;JavaUtilJarClassLibrary"/>
		<rdfs:subClassOf rdf:resource="&java-se-6;JavaUtilSpiClassLibrary"/>
		<rdfs:subClassOf rdf:resource="&java-se-6;JavaUtilConcurrentClassLibrary"/>
		<rdfs:subClassOf rdf:resource="&java-se-6;JavaUtilConcurrentAtomicClassLibrary"/>
		<rdfs:subClassOf rdf:resource="&java-se-6;JavaUtilConcurrentLocksClassLibrary"/>
		<rdfs:subClassOf rdf:resource="&java-se-6;JavaUtilZipClassLibrary"/>
		<rdfs:subClassOf rdf:resource="&java-se-6;JavaUtilLoggingClassLibrary"/>
		<rdfs:subClassOf rdf:resource="&java-se-6;JavaUtilPrefsClassLibrary"/>
		<rdfs:subClassOf rdf:resource="&java-se-6;JavaUtilRegexClassLibrary"/>
		<rdfs:subClassOf rdf:resource="&java-se-6;JavaAppletClassLibrary"/>
		<rdfs:subClassOf rdf:resource="&java-se-6;JavaBeansClassLibrary"/>
		<rdfs:subClassOf rdf:resource="&java-se-6;JavaBeansBeancontextClassLibrary"/>
		<rdfs:subClassOf rdf:resource="&java-se-6;JavaTextClassLibrary"/>
		<rdfs:subClassOf rdf:resource="&java-se-6;JavaTextSpiClassLibrary"/>
		<rdfs:subClassOf rdf:resource="&java-se-6;JavaRmiClassLibrary"/>
		<rdfs:subClassOf rdf:resource="&java-se-6;JavaRmiActivationClassLibrary"/>
		<rdfs:subClassOf rdf:resource="&java-se-6;JavaRmiServerClassLibrary"/>
		<rdfs:subClassOf rdf:resource="&java-se-6;JavaRmiDgcClassLibrary"/>
		<rdfs:subClassOf rdf:resource="&java-se-6;JavaRmiRegistryClassLibrary"/>
		<rdfs:subClassOf rdf:resource="&java-se-6;JavaSqlClassLibrary"/>
		<rdfs:subClassOf rdf:resource="&java-se-6;OrgW3cDomClassLibrary"/>
		<rdfs:subClassOf rdf:resource="&java-se-6;OrgW3cDomLsClassLibrary"/>
		<rdfs:subClassOf rdf:resource="&java-se-6;OrgW3cDomBootstrapClassLibrary"/>
		<rdfs:subClassOf rdf:resource="&java-se-6;OrgW3cDomCssClassLibrary"/>
		<rdfs:subClassOf rdf:resource="&java-se-6;OrgW3cDomStylesheetsClassLibrary"/>
		<rdfs:subClassOf rdf:resource="&java-se-6;OrgW3cDomViewsClassLibrary"/>
		<rdfs:subClassOf rdf:resource="&java-se-6;OrgW3cDomEventsClassLibrary"/>
		<rdfs:subClassOf rdf:resource="&java-se-6;OrgW3cDomHtmlClassLibrary"/>
		<rdfs:subClassOf rdf:resource="&java-se-6;OrgW3cDomTraversalClassLibrary"/>
		<rdfs:subClassOf rdf:resource="&java-se-6;OrgW3cDomRangesClassLibrary"/>
		<rdfs:subClassOf rdf:resource="&java-se-6;OrgW3cDomXpathClassLibrary"/>
		<rdfs:subClassOf rdf:resource="&java-se-6;OrgOmgCORBA_2_3ClassLibrary"/>
		<rdfs:subClassOf rdf:resource="&java-se-6;OrgOmgCORBA_2_3PortableClassLibrary"/>
		<rdfs:subClassOf rdf:resource="&java-se-6;OrgOmgCORBAClassLibrary"/>
		<rdfs:subClassOf rdf:resource="&java-se-6;OrgOmgCORBAPortableClassLibrary"/>
		<rdfs:subClassOf rdf:resource="&java-se-6;OrgOmgCORBADynAnyPackageClassLibrary"/>
		<rdfs:subClassOf rdf:resource="&java-se-6;OrgOmgCORBAORBPackageClassLibrary"/>
		<rdfs:subClassOf rdf:resource="&java-se-6;OrgOmgCORBATypeCodePackageClassLibrary"/>
		<rdfs:subClassOf rdf:resource="&java-se-6;OrgOmgSendingContextClassLibrary"/>
		<rdfs:subClassOf rdf:resource="&java-se-6;OrgOmgCosNamingClassLibrary"/>
		<rdfs:subClassOf rdf:resource="&java-se-6;OrgOmgCosNamingNamingContextExtPackageClassLibrary"/>
		<rdfs:subClassOf rdf:resource="&java-se-6;OrgOmgCosNamingNamingContextPackageClassLibrary"/>
		<rdfs:subClassOf rdf:resource="&java-se-6;OrgOmgPortableServerClassLibrary"/>
		<rdfs:subClassOf rdf:resource="&java-se-6;OrgOmgPortableServerCurrentPackageClassLibrary"/>
		<rdfs:subClassOf rdf:resource="&java-se-6;OrgOmgPortableServerPOAManagerPackageClassLibrary"/>
		<rdfs:subClassOf rdf:resource="&java-se-6;OrgOmgPortableServerPOAPackageClassLibrary"/>
		<rdfs:subClassOf rdf:resource="&java-se-6;OrgOmgPortableServerPortableClassLibrary"/>
		<rdfs:subClassOf rdf:resource="&java-se-6;OrgOmgPortableServerServantLocatorPackageClassLibrary"/>
		<rdfs:subClassOf rdf:resource="&java-se-6;OrgOmgDynamicClassLibrary"/>
		<rdfs:subClassOf rdf:resource="&java-se-6;OrgOmgDynamicAnyClassLibrary"/>
		<rdfs:subClassOf rdf:resource="&java-se-6;OrgOmgDynamicAnyDynAnyFactoryPackageClassLibrary"/>
		<rdfs:subClassOf rdf:resource="&java-se-6;OrgOmgDynamicAnyDynAnyPackageClassLibrary"/>
		<rdfs:subClassOf rdf:resource="&java-se-6;OrgOmgIOPClassLibrary"/>
		<rdfs:subClassOf rdf:resource="&java-se-6;OrgOmgIOPCodecFactoryPackageClassLibrary"/>
		<rdfs:subClassOf rdf:resource="&java-se-6;OrgOmgIOPCodecPackageClassLibrary"/>
		<rdfs:subClassOf rdf:resource="&java-se-6;OrgOmgMessagingClassLibrary"/>
		<rdfs:subClassOf rdf:resource="&java-se-6;OrgOmgPortableInterceptorClassLibrary"/>
		<rdfs:subClassOf rdf:resource="&java-se-6;OrgOmgPortableInterceptorORBInitInfoPackageClassLibrary"/>
		<rdfs:subClassOf rdf:resource="&java-se-6;OrgOmgStubJavaRmiClassLibrary"/>
		<rdfs:subClassOf rdf:resource="&java-se-6;OrgOmgStubJavaxManagementRemoteRmiClassLibrary"/>
		<rdfs:subClassOf rdf:resource="&java-se-6;OrgXmlSaxClassLibrary"/>
		<rdfs:subClassOf rdf:resource="&java-se-6;OrgXmlSaxHelpersClassLibrary"/>
		<rdfs:subClassOf rdf:resource="&java-se-6;OrgXmlSaxExtClassLibrary"/>
		<rdfs:subClassOf rdf:resource="&java-se-6;OrgIetfJgssClassLibrary"/>
		<rdfs:comment xml:lang="en">Java class library implementing the Java SE 6 API</rdfs:comment>
		<rdfs:comment xml:lang="OWLManchester">platform:implementsInterface some JavaSE6API</rdfs:comment>
	</owl:Class>
	<owl:Class rdf:about="&java-se-6;JavaSE6BytecodeFormat">
		<rdfs:subClassOf rdf:resource="&j2se-5_0;J2SE5_0BytecodeFormat"/>
		<rdfs:comment xml:lang="en">Java SE 6 bytecode format</rdfs:comment>
		<rdfs:comment xml:lang="OWLManchester">java:majorVersionNumber some xsd:integer[>="50"^^xsd:integer] and java:preverified value false</rdfs:comment>
	</owl:Class>
	<java-se-6:JavaSE6BytecodeFormat rdf:about="&java-se-6;theJavaSE6BytecodeFormat">
		<java:preverified rdf:datatype="http://www.w3.org/2001/XMLSchema#boolean">false</java:preverified>
		<java:minorVersionNumber rdf:datatype="http://www.w3.org/2001/XMLSchema#integer">0</java:minorVersionNumber>
		<java:majorVersionNumber rdf:datatype="http://www.w3.org/2001/XMLSchema#integer">50</java:majorVersionNumber>
	</java-se-6:JavaSE6BytecodeFormat>
	<java-se-6:JavaSE6API rdf:about="&java-se-6;theJavaSE6API">
		<platform:comprisesInterfacePart rdf:resource="&java-se-6;theOrgIetfJgssPart"/>
		<platform:comprisesInterfacePart rdf:resource="&java-se-6;theOrgXmlSaxExtPart"/>
		<platform:comprisesInterfacePart rdf:resource="&java-se-6;theOrgXmlSaxHelpersPart"/>
		<platform:comprisesInterfacePart rdf:resource="&java-se-6;theOrgXmlSaxPart"/>
		<platform:comprisesInterfacePart rdf:resource="&java-se-6;theOrgOmgStubJavaxManagementRemoteRmiPart"/>
		<platform:comprisesInterfacePart rdf:resource="&java-se-6;theOrgOmgStubJavaRmiPart"/>
		<platform:comprisesInterfacePart rdf:resource="&java-se-6;theOrgOmgPortableInterceptorORBInitInfoPackagePart"/>
		<platform:comprisesInterfacePart rdf:resource="&java-se-6;theOrgOmgPortableInterceptorPart"/>
		<platform:comprisesInterfacePart rdf:resource="&java-se-6;theOrgOmgMessagingPart"/>
		<platform:comprisesInterfacePart rdf:resource="&java-se-6;theOrgOmgIOPCodecPackagePart"/>
		<platform:comprisesInterfacePart rdf:resource="&java-se-6;theOrgOmgIOPCodecFactoryPackagePart"/>
		<platform:comprisesInterfacePart rdf:resource="&java-se-6;theOrgOmgIOPPart"/>
		<platform:comprisesInterfacePart rdf:resource="&java-se-6;theOrgOmgDynamicAnyDynAnyPackagePart"/>
		<platform:comprisesInterfacePart rdf:resource="&java-se-6;theOrgOmgDynamicAnyDynAnyFactoryPackagePart"/>
		<platform:comprisesInterfacePart rdf:resource="&java-se-6;theOrgOmgDynamicAnyPart"/>
		<platform:comprisesInterfacePart rdf:resource="&java-se-6;theOrgOmgDynamicPart"/>
		<platform:comprisesInterfacePart rdf:resource="&java-se-6;theOrgOmgPortableServerServantLocatorPackagePart"/>
		<platform:comprisesInterfacePart rdf:resource="&java-se-6;theOrgOmgPortableServerPortablePart"/>
		<platform:comprisesInterfacePart rdf:resource="&java-se-6;theOrgOmgPortableServerPOAPackagePart"/>
		<platform:comprisesInterfacePart rdf:resource="&java-se-6;theOrgOmgPortableServerPOAManagerPackagePart"/>
		<platform:comprisesInterfacePart rdf:resource="&java-se-6;theOrgOmgPortableServerCurrentPackagePart"/>
		<platform:comprisesInterfacePart rdf:resource="&java-se-6;theOrgOmgPortableServerPart"/>
		<platform:comprisesInterfacePart rdf:resource="&java-se-6;theOrgOmgCosNamingNamingContextPackagePart"/>
		<platform:comprisesInterfacePart rdf:resource="&java-se-6;theOrgOmgCosNamingNamingContextExtPackagePart"/>
		<platform:comprisesInterfacePart rdf:resource="&java-se-6;theOrgOmgCosNamingPart"/>
		<platform:comprisesInterfacePart rdf:resource="&java-se-6;theOrgOmgSendingContextPart"/>
		<platform:comprisesInterfacePart rdf:resource="&java-se-6;theOrgOmgCORBATypeCodePackagePart"/>
		<platform:comprisesInterfacePart rdf:resource="&java-se-6;theOrgOmgCORBAORBPackagePart"/>
		<platform:comprisesInterfacePart rdf:resource="&java-se-6;theOrgOmgCORBADynAnyPackagePart"/>
		<platform:comprisesInterfacePart rdf:resource="&java-se-6;theOrgOmgCORBAPortablePart"/>
		<platform:comprisesInterfacePart rdf:resource="&java-se-6;theOrgOmgCORBAPart"/>
		<platform:comprisesInterfacePart rdf:resource="&java-se-6;theOrgOmgCORBA_2_3PortablePart"/>
		<platform:comprisesInterfacePart rdf:resource="&java-se-6;theOrgOmgCORBA_2_3Part"/>
		<platform:comprisesInterfacePart rdf:resource="&java-se-6;theOrgW3cDomXpathPart"/>
		<platform:comprisesInterfacePart rdf:resource="&java-se-6;theOrgW3cDomRangesPart"/>
		<platform:comprisesInterfacePart rdf:resource="&java-se-6;theOrgW3cDomTraversalPart"/>
		<platform:comprisesInterfacePart rdf:resource="&java-se-6;theOrgW3cDomHtmlPart"/>
		<platform:comprisesInterfacePart rdf:resource="&java-se-6;theOrgW3cDomEventsPart"/>
		<platform:comprisesInterfacePart rdf:resource="&java-se-6;theOrgW3cDomViewsPart"/>
		<platform:comprisesInterfacePart rdf:resource="&java-se-6;theOrgW3cDomStylesheetsPart"/>
		<platform:comprisesInterfacePart rdf:resource="&java-se-6;theOrgW3cDomCssPart"/>
		<platform:comprisesInterfacePart rdf:resource="&java-se-6;theOrgW3cDomBootstrapPart"/>
		<platform:comprisesInterfacePart rdf:resource="&java-se-6;theOrgW3cDomLsPart"/>
		<platform:comprisesInterfacePart rdf:resource="&java-se-6;theOrgW3cDomPart"/>
		<platform:comprisesInterfacePart rdf:resource="&java-se-6;theJavaSqlPart"/>
		<platform:comprisesInterfacePart rdf:resource="&java-se-6;theJavaRmiRegistryPart"/>
		<platform:comprisesInterfacePart rdf:resource="&java-se-6;theJavaRmiDgcPart"/>
		<platform:comprisesInterfacePart rdf:resource="&java-se-6;theJavaRmiServerPart"/>
		<platform:comprisesInterfacePart rdf:resource="&java-se-6;theJavaRmiActivationPart"/>
		<platform:comprisesInterfacePart rdf:resource="&java-se-6;theJavaRmiPart"/>
		<platform:comprisesInterfacePart rdf:resource="&java-se-6;theJavaTextSpiPart"/>
		<platform:comprisesInterfacePart rdf:resource="&java-se-6;theJavaTextPart"/>
		<platform:comprisesInterfacePart rdf:resource="&java-se-6;theJavaBeansBeancontextPart"/>
		<platform:comprisesInterfacePart rdf:resource="&java-se-6;theJavaBeansPart"/>
		<platform:comprisesInterfacePart rdf:resource="&java-se-6;theJavaAppletPart"/>
		<platform:comprisesInterfacePart rdf:resource="&java-se-6;theJavaUtilRegexPart"/>
		<platform:comprisesInterfacePart rdf:resource="&java-se-6;theJavaUtilPrefsPart"/>
		<platform:comprisesInterfacePart rdf:resource="&java-se-6;theJavaUtilLoggingPart"/>
		<platform:comprisesInterfacePart rdf:resource="&java-se-6;theJavaUtilZipPart"/>
		<platform:comprisesInterfacePart rdf:resource="&java-se-6;theJavaUtilConcurrentLocksPart"/>
		<platform:comprisesInterfacePart rdf:resource="&java-se-6;theJavaUtilConcurrentAtomicPart"/>
		<platform:comprisesInterfacePart rdf:resource="&java-se-6;theJavaUtilConcurrentPart"/>
		<platform:comprisesInterfacePart rdf:resource="&java-se-6;theJavaUtilSpiPart"/>
		<platform:comprisesInterfacePart rdf:resource="&java-se-6;theJavaUtilJarPart"/>
		<platform:comprisesInterfacePart rdf:resource="&java-se-6;theJavaUtilPart"/>
		<platform:comprisesInterfacePart rdf:resource="&java-se-6;theJavaNioCharsetSpiPart"/>
		<platform:comprisesInterfacePart rdf:resource="&java-se-6;theJavaNioCharsetPart"/>
		<platform:comprisesInterfacePart rdf:resource="&java-se-6;theJavaNioChannelsSpiPart"/>
		<platform:comprisesInterfacePart rdf:resource="&java-se-6;theJavaNioChannelsPart"/>
		<platform:comprisesInterfacePart rdf:resource="&java-se-6;theJavaNioPart"/>
		<platform:comprisesInterfacePart rdf:resource="&java-se-6;theJavaMathPart"/>
		<platform:comprisesInterfacePart rdf:resource="&java-se-6;theJavaSecurityInterfacesPart"/>
		<platform:comprisesInterfacePart rdf:resource="&java-se-6;theJavaSecurityAclPart"/>
		<platform:comprisesInterfacePart rdf:resource="&java-se-6;theJavaSecurityCertPart"/>
		<platform:comprisesInterfacePart rdf:resource="&java-se-6;theJavaSecuritySpecPart"/>
		<platform:comprisesInterfacePart rdf:resource="&java-se-6;theJavaSecurityPart"/>
		<platform:comprisesInterfacePart rdf:resource="&java-se-6;theJavaIoPart"/>
		<platform:comprisesInterfacePart rdf:resource="&java-se-6;theJavaNetPart"/>
		<platform:comprisesInterfacePart rdf:resource="&java-se-6;theJavaAwtFontPart"/>
		<platform:comprisesInterfacePart rdf:resource="&java-se-6;theJavaAwtDndPart"/>
		<platform:comprisesInterfacePart rdf:resource="&java-se-6;theJavaAwtColorPart"/>
		<platform:comprisesInterfacePart rdf:resource="&java-se-6;theJavaAwtImSpiPart"/>
		<platform:comprisesInterfacePart rdf:resource="&java-se-6;theJavaAwtImPart"/>
		<platform:comprisesInterfacePart rdf:resource="&java-se-6;theJavaAwtGeomPart"/>
		<platform:comprisesInterfacePart rdf:resource="&java-se-6;theJavaAwtImageRenderablePart"/>
		<platform:comprisesInterfacePart rdf:resource="&java-se-6;theJavaAwtImagePart"/>
		<platform:comprisesInterfacePart rdf:resource="&java-se-6;theJavaAwtEventPart"/>
		<platform:comprisesInterfacePart rdf:resource="&java-se-6;theJavaAwtDatatransferPart"/>
		<platform:comprisesInterfacePart rdf:resource="&java-se-6;theJavaAwtPrintPart"/>
		<platform:comprisesInterfacePart rdf:resource="&java-se-6;theJavaAwtPart"/>
		<platform:comprisesInterfacePart rdf:resource="&java-se-6;theJavaLangRefPart"/>
		<platform:comprisesInterfacePart rdf:resource="&java-se-6;theJavaLangManagementPart"/>
		<platform:comprisesInterfacePart rdf:resource="&java-se-6;theJavaLangInstrumentPart"/>
		<platform:comprisesInterfacePart rdf:resource="&java-se-6;theJavaLangReflectPart"/>
		<platform:comprisesInterfacePart rdf:resource="&java-se-6;theJavaLangAnnotationPart"/>
		<platform:comprisesInterfacePart rdf:resource="&java-se-6;theJavaLangPart"/>
		<platform:comprisesInterfacePart rdf:resource="&java-se-6;theJavaxTransactionXaPart"/>
		<platform:comprisesInterfacePart rdf:resource="&java-se-6;theJavaxTransactionPart"/>
		<platform:comprisesInterfacePart rdf:resource="&java-se-6;theJavaxSqlRowsetSerialPart"/>
		<platform:comprisesInterfacePart rdf:resource="&java-se-6;theJavaxSqlRowsetSpiPart"/>
		<platform:comprisesInterfacePart rdf:resource="&java-se-6;theJavaxSqlRowsetPart"/>
		<platform:comprisesInterfacePart rdf:resource="&java-se-6;theJavaxSqlPart"/>
		<platform:comprisesInterfacePart rdf:resource="&java-se-6;theJavaxSoundSampledSpiPart"/>
		<platform:comprisesInterfacePart rdf:resource="&java-se-6;theJavaxSoundSampledPart"/>
		<platform:comprisesInterfacePart rdf:resource="&java-se-6;theJavaxSoundMidiSpiPart"/>
		<platform:comprisesInterfacePart rdf:resource="&java-se-6;theJavaxSoundMidiPart"/>
		<platform:comprisesInterfacePart rdf:resource="&java-se-6;theJavaxSmartcardioPart"/>
		<platform:comprisesInterfacePart rdf:resource="&java-se-6;theJavaxScriptPart"/>
		<platform:comprisesInterfacePart rdf:resource="&java-se-6;theJavaxPrintEventPart"/>
		<platform:comprisesInterfacePart rdf:resource="&java-se-6;theJavaxPrintAttributeStandardPart"/>
		<platform:comprisesInterfacePart rdf:resource="&java-se-6;theJavaxPrintAttributePart"/>
		<platform:comprisesInterfacePart rdf:resource="&java-se-6;theJavaxPrintPart"/>
		<platform:comprisesInterfacePart rdf:resource="&java-se-6;theJavaxNamingSpiPart"/>
		<platform:comprisesInterfacePart rdf:resource="&java-se-6;theJavaxNamingLdapPart"/>
		<platform:comprisesInterfacePart rdf:resource="&java-se-6;theJavaxNamingEventPart"/>
		<platform:comprisesInterfacePart rdf:resource="&java-se-6;theJavaxNamingDirectoryPart"/>
		<platform:comprisesInterfacePart rdf:resource="&java-se-6;theJavaxNamingPart"/>
		<platform:comprisesInterfacePart rdf:resource="&java-se-6;theJavaxRmiSslPart"/>
		<platform:comprisesInterfacePart rdf:resource="&java-se-6;theJavaxRmiCORBAPart"/>
		<platform:comprisesInterfacePart rdf:resource="&java-se-6;theJavaxRmiPart"/>
		<platform:comprisesInterfacePart rdf:resource="&java-se-6;theJavaxJwsSoapPart"/>
		<platform:comprisesInterfacePart rdf:resource="&java-se-6;theJavaxJwsPart"/>
		<platform:comprisesInterfacePart rdf:resource="&java-se-6;theJavaxImageioPluginsJpegPart"/>
		<platform:comprisesInterfacePart rdf:resource="&java-se-6;theJavaxImageioPluginsBmpPart"/>
		<platform:comprisesInterfacePart rdf:resource="&java-se-6;theJavaxImageioEventPart"/>
		<platform:comprisesInterfacePart rdf:resource="&java-se-6;theJavaxImageioSpiPart"/>
		<platform:comprisesInterfacePart rdf:resource="&java-se-6;theJavaxImageioStreamPart"/>
		<platform:comprisesInterfacePart rdf:resource="&java-se-6;theJavaxImageioMetadataPart"/>
		<platform:comprisesInterfacePart rdf:resource="&java-se-6;theJavaxImageioPart"/>
		<platform:comprisesInterfacePart rdf:resource="&java-se-6;theJavaxToolsPart"/>
		<platform:comprisesInterfacePart rdf:resource="&java-se-6;theJavaxLangModelTypePart"/>
		<platform:comprisesInterfacePart rdf:resource="&java-se-6;theJavaxLangModelUtilPart"/>
		<platform:comprisesInterfacePart rdf:resource="&java-se-6;theJavaxLangModelElementPart"/>
		<platform:comprisesInterfacePart rdf:resource="&java-se-6;theJavaxLangModelPart"/>
		<platform:comprisesInterfacePart rdf:resource="&java-se-6;theJavaxAnnotationProcessingPart"/>
		<platform:comprisesInterfacePart rdf:resource="&java-se-6;theJavaxAnnotationPart"/>
		<platform:comprisesInterfacePart rdf:resource="&java-se-6;theJavaxActivityPart"/>
		<platform:comprisesInterfacePart rdf:resource="&java-se-6;theJavaxActivationPart"/>
		<platform:comprisesInterfacePart rdf:resource="&java-se-6;theJavaxXmlXpathPart"/>
		<platform:comprisesInterfacePart rdf:resource="&java-se-6;theJavaxXmlWsWsaddressingPart"/>
		<platform:comprisesInterfacePart rdf:resource="&java-se-6;theJavaxXmlWsSpiPart"/>
		<platform:comprisesInterfacePart rdf:resource="&java-se-6;theJavaxXmlWsSoapPart"/>
		<platform:comprisesInterfacePart rdf:resource="&java-se-6;theJavaxXmlWsHttpPart"/>
		<platform:comprisesInterfacePart rdf:resource="&java-se-6;theJavaxXmlWsHandlerSoapPart"/>
		<platform:comprisesInterfacePart rdf:resource="&java-se-6;theJavaxXmlWsHandlerPart"/>
		<platform:comprisesInterfacePart rdf:resource="&java-se-6;theJavaxXmlWsPart"/>
		<platform:comprisesInterfacePart rdf:resource="&java-se-6;theJavaxXmlSoapPart"/>
		<platform:comprisesInterfacePart rdf:resource="&java-se-6;theJavaxXmlDatatypePart"/>
		<platform:comprisesInterfacePart rdf:resource="&java-se-6;theJavaxXmlCryptoDomPart"/>
		<platform:comprisesInterfacePart rdf:resource="&java-se-6;theJavaxXmlCryptoDsigDomPart"/>
		<platform:comprisesInterfacePart rdf:resource="&java-se-6;theJavaxXmlCryptoDsigSpecPart"/>
		<platform:comprisesInterfacePart rdf:resource="&java-se-6;theJavaxXmlCryptoDsigKeyinfoPart"/>
		<platform:comprisesInterfacePart rdf:resource="&java-se-6;theJavaxXmlCryptoDsigPart"/>
		<platform:comprisesInterfacePart rdf:resource="&java-se-6;theJavaxXmlCryptoPart"/>
		<platform:comprisesInterfacePart rdf:resource="&java-se-6;theJavaxXmlParsersPart"/>
		<platform:comprisesInterfacePart rdf:resource="&java-se-6;theJavaxXmlStreamUtilPart"/>
		<platform:comprisesInterfacePart rdf:resource="&java-se-6;theJavaxXmlStreamEventsPart"/>
		<platform:comprisesInterfacePart rdf:resource="&java-se-6;theJavaxXmlStreamPart"/>
		<platform:comprisesInterfacePart rdf:resource="&java-se-6;theJavaxXmlNamespacePart"/>
		<platform:comprisesInterfacePart rdf:resource="&java-se-6;theJavaxXmlValidationPart"/>
		<platform:comprisesInterfacePart rdf:resource="&java-se-6;theJavaxXmlBindUtilPart"/>
		<platform:comprisesInterfacePart rdf:resource="&java-se-6;theJavaxXmlBindHelpersPart"/>
		<platform:comprisesInterfacePart rdf:resource="&java-se-6;theJavaxXmlBindAttachmentPart"/>
		<platform:comprisesInterfacePart rdf:resource="&java-se-6;theJavaxXmlBindAnnotationAdaptersPart"/>
		<platform:comprisesInterfacePart rdf:resource="&java-se-6;theJavaxXmlBindAnnotationPart"/>
		<platform:comprisesInterfacePart rdf:resource="&java-se-6;theJavaxXmlBindPart"/>
		<platform:comprisesInterfacePart rdf:resource="&java-se-6;theJavaxXmlTransformStreamPart"/>
		<platform:comprisesInterfacePart rdf:resource="&java-se-6;theJavaxXmlTransformStaxPart"/>
		<platform:comprisesInterfacePart rdf:resource="&java-se-6;theJavaxXmlTransformSaxPart"/>
		<platform:comprisesInterfacePart rdf:resource="&java-se-6;theJavaxXmlTransformDomPart"/>
		<platform:comprisesInterfacePart rdf:resource="&java-se-6;theJavaxXmlTransformPart"/>
		<platform:comprisesInterfacePart rdf:resource="&java-se-6;theJavaxXmlPart"/>
		<platform:comprisesInterfacePart rdf:resource="&java-se-6;theJavaxManagementTimerPart"/>
		<platform:comprisesInterfacePart rdf:resource="&java-se-6;theJavaxManagementRemoteRmiPart"/>
		<platform:comprisesInterfacePart rdf:resource="&java-se-6;theJavaxManagementRemotePart"/>
		<platform:comprisesInterfacePart rdf:resource="&java-se-6;theJavaxManagementRelationPart"/>
		<platform:comprisesInterfacePart rdf:resource="&java-se-6;theJavaxManagementMonitorPart"/>
		<platform:comprisesInterfacePart rdf:resource="&java-se-6;theJavaxManagementModelmbeanPart"/>
		<platform:comprisesInterfacePart rdf:resource="&java-se-6;theJavaxManagementLoadingPart"/>
		<platform:comprisesInterfacePart rdf:resource="&java-se-6;theJavaxManagementOpenmbeanPart"/>
		<platform:comprisesInterfacePart rdf:resource="&java-se-6;theJavaxManagementPart"/>
		<platform:comprisesInterfacePart rdf:resource="&java-se-6;theJavaxSwingUndoPart"/>
		<platform:comprisesInterfacePart rdf:resource="&java-se-6;theJavaxSwingTablePart"/>
		<platform:comprisesInterfacePart rdf:resource="&java-se-6;theJavaxSwingBorderPart"/>
		<platform:comprisesInterfacePart rdf:resource="&java-se-6;theJavaxSwingTreePart"/>
		<platform:comprisesInterfacePart rdf:resource="&java-se-6;theJavaxSwingFilechooserPart"/>
		<platform:comprisesInterfacePart rdf:resource="&java-se-6;theJavaxSwingPlafSynthPart"/>
		<platform:comprisesInterfacePart rdf:resource="&java-se-6;theJavaxSwingPlafMultiPart"/>
		<platform:comprisesInterfacePart rdf:resource="&java-se-6;theJavaxSwingPlafMetalPart"/>
		<platform:comprisesInterfacePart rdf:resource="&java-se-6;theJavaxSwingPlafBasicPart"/>
		<platform:comprisesInterfacePart rdf:resource="&java-se-6;theJavaxSwingPlafPart"/>
		<platform:comprisesInterfacePart rdf:resource="&java-se-6;theJavaxSwingColorchooserPart"/>
		<platform:comprisesInterfacePart rdf:resource="&java-se-6;theJavaxSwingEventPart"/>
		<platform:comprisesInterfacePart rdf:resource="&java-se-6;theJavaxSwingTextRtfPart"/>
		<platform:comprisesInterfacePart rdf:resource="&java-se-6;theJavaxSwingTextHtmlParserPart"/>
		<platform:comprisesInterfacePart rdf:resource="&java-se-6;theJavaxSwingTextHtmlPart"/>
		<platform:comprisesInterfacePart rdf:resource="&java-se-6;theJavaxSwingTextPart"/>
		<platform:comprisesInterfacePart rdf:resource="&java-se-6;theJavaxSwingPart"/>
		<platform:comprisesInterfacePart rdf:resource="&java-se-6;theJavaxAccessibilityPart"/>
		<platform:comprisesInterfacePart rdf:resource="&java-se-6;theJavaxSecuritySaslPart"/>
		<platform:comprisesInterfacePart rdf:resource="&java-se-6;theJavaxSecurityAuthSpiPart"/>
		<platform:comprisesInterfacePart rdf:resource="&java-se-6;theJavaxSecurityAuthKerberosPart"/>
		<platform:comprisesInterfacePart rdf:resource="&java-se-6;theJavaxSecurityAuthX500Part"/>
		<platform:comprisesInterfacePart rdf:resource="&java-se-6;theJavaxSecurityAuthLoginPart"/>
		<platform:comprisesInterfacePart rdf:resource="&java-se-6;theJavaxSecurityAuthCallbackPart"/>
		<platform:comprisesInterfacePart rdf:resource="&java-se-6;theJavaxSecurityAuthPart"/>
		<platform:comprisesInterfacePart rdf:resource="&java-se-6;theJavaxSecurityCertPart"/>
		<platform:comprisesInterfacePart rdf:resource="&java-se-6;theJavaxNetSslPart"/>
		<platform:comprisesInterfacePart rdf:resource="&java-se-6;theJavaxNetPart"/>
		<platform:comprisesInterfacePart rdf:resource="&java-se-6;theJavaxCryptoSpecPart"/>
		<platform:comprisesInterfacePart rdf:resource="&java-se-6;theJavaxCryptoInterfacesPart"/>
		<platform:comprisesInterfacePart rdf:resource="&java-se-6;theJavaxCryptoPart"/>
		<platform:comprisesInterfacePart rdf:resource="&java-se-6;theJavaxJnlpPart"/>
	</java-se-6:JavaSE6API>
	<owl:Class rdf:about="&java-se-6;JavaSE6VM">
		<owl:equivalentClass>
			<owl:Restriction>
				<owl:onProperty rdf:resource="&platform;implementsInterface"/>
				<owl:someValuesFrom rdf:resource="&java-se-6;JavaSE6BytecodeFormat"/>
			</owl:Restriction>
		</owl:equivalentClass>
		<rdfs:subClassOf rdf:resource="&java;JavaVM"/>
		<rdfs:comment xml:lang="en">Java SE 6 virtual machine</rdfs:comment>
	</owl:Class>
	<owl:Class rdf:about="&java-se-6;JavaSE6JRE">
		<owl:equivalentClass>
			<owl:Class >
				<owl:intersectionOf rdf:parseType="Collection">
					<owl:Restriction>
						<owl:onProperty rdf:resource="&platform;providesFeature"/>
						<owl:someValuesFrom rdf:resource="&java-se-6;JavaSE6ClassLibrary"/>
					</owl:Restriction>
					<owl:Restriction>
						<owl:onProperty rdf:resource="&platform;providesFeature"/>
						<owl:someValuesFrom rdf:resource="&java-se-6;JavaSE6VM"/>
					</owl:Restriction>
				</owl:intersectionOf>
			</owl:Class>
		</owl:equivalentClass>
		<rdfs:subClassOf rdf:resource="&java;JRE"/>
		<rdfs:comment xml:lang="en">Java SE 6 Java Runtime Environment</rdfs:comment>
	</owl:Class>
	<owl:Class rdf:about="&java-se-6;JavaxJnlp">
		<rdfs:subClassOf rdf:resource="&java;JavaAPIPart"/>
		<rdfs:seeAlso rdf:resource="&java-se-6;JavaAwtDatatransfer"/>
		<rdfs:seeAlso rdf:resource="&java-se-6;JavaLang"/>
		<rdfs:seeAlso rdf:resource="&java-se-6;JavaAwtPrint"/>
		<rdfs:seeAlso rdf:resource="&java-se-6;JavaIo"/>
		<rdfs:seeAlso rdf:resource="&java-se-6;JavaNet"/>
		<rdfs:comment xml:lang="en">Java API part implementing the javax.jnlp package for Java SE 6</rdfs:comment>
	</owl:Class>
	<owl:Class rdf:about="&java-se-6;JavaxCrypto">
		<owl:equivalentClass rdf:resource="&j2se-5_0;JavaxCrypto"/>
		<rdfs:subClassOf rdf:resource="&java;JavaAPIPart"/>
		<rdfs:seeAlso rdf:resource="&java-se-6;JavaSecuritySpec"/>
		<rdfs:seeAlso rdf:resource="&java-se-6;JavaLang"/>
		<rdfs:seeAlso rdf:resource="&java-se-6;JavaNio"/>
		<rdfs:seeAlso rdf:resource="&java-se-6;JavaSecurity"/>
		<rdfs:seeAlso rdf:resource="&java-se-6;JavaIo"/>
		<rdfs:seeAlso rdf:resource="&java-se-6;JavaSecurityCert"/>
		<rdfs:comment xml:lang="en">Java API part implementing the javax.crypto package for Java SE 6</rdfs:comment>
	</owl:Class>
	<owl:Class rdf:about="&java-se-6;JavaxCryptoInterfaces">
		<owl:equivalentClass rdf:resource="&j2se-5_0;JavaxCryptoInterfaces"/>
		<rdfs:subClassOf rdf:resource="&java;JavaAPIPart"/>
		<rdfs:seeAlso rdf:resource="&java-se-6;JavaxCryptoSpec"/>
		<rdfs:seeAlso rdf:resource="&java-se-6;JavaMath"/>
		<rdfs:seeAlso rdf:resource="&java-se-6;JavaSecurity"/>
		<rdfs:seeAlso rdf:resource="&java-se-6;JavaxCrypto"/>
		<rdfs:comment xml:lang="en">Java API part implementing the javax.crypto.interfaces package for Java SE 6</rdfs:comment>
	</owl:Class>
	<owl:Class rdf:about="&java-se-6;JavaxCryptoSpec">
		<owl:equivalentClass rdf:resource="&j2se-5_0;JavaxCryptoSpec"/>
		<rdfs:subClassOf rdf:resource="&java;JavaAPIPart"/>
		<rdfs:seeAlso rdf:resource="&java-se-6;JavaSecuritySpec"/>
		<rdfs:seeAlso rdf:resource="&java-se-6;JavaMath"/>
		<rdfs:seeAlso rdf:resource="&java-se-6;JavaLang"/>
		<rdfs:seeAlso rdf:resource="&java-se-6;JavaxCrypto"/>
		<rdfs:comment xml:lang="en">Java API part implementing the javax.crypto.spec package for Java SE 6</rdfs:comment>
	</owl:Class>
	<owl:Class rdf:about="&java-se-6;JavaxNet">
		<owl:equivalentClass rdf:resource="&j2se-5_0;JavaxNet"/>
		<rdfs:subClassOf rdf:resource="&java;JavaAPIPart"/>
		<rdfs:seeAlso rdf:resource="&java-se-6;JavaNet"/>
		<rdfs:seeAlso rdf:resource="&java-se-6;JavaLang"/>
		<rdfs:comment xml:lang="en">Java API part implementing the javax.net package for Java SE 6</rdfs:comment>
	</owl:Class>
	<owl:Class rdf:about="&java-se-6;JavaxNetSsl">
		<rdfs:subClassOf rdf:resource="&j2se-5_0;JavaxNetSsl"/>
		<rdfs:seeAlso rdf:resource="&java-se-6;JavaLang"/>
		<rdfs:seeAlso rdf:resource="&java-se-6;JavaNio"/>
		<rdfs:seeAlso rdf:resource="&java-se-6;JavaIo"/>
		<rdfs:seeAlso rdf:resource="&java-se-6;JavaUtil"/>
		<rdfs:seeAlso rdf:resource="&java-se-6;JavaSecurity"/>
		<rdfs:seeAlso rdf:resource="&java-se-6;JavaxNet"/>
		<rdfs:seeAlso rdf:resource="&java-se-6;JavaNet"/>
		<rdfs:seeAlso rdf:resource="&java-se-6;JavaSecurityCert"/>
		<rdfs:comment xml:lang="en">Java API part implementing the javax.net.ssl package for Java SE 6</rdfs:comment>
	</owl:Class>
	<owl:Class rdf:about="&java-se-6;JavaxSecurityCert">
		<owl:equivalentClass rdf:resource="&j2se-5_0;JavaxSecurityCert"/>
		<rdfs:subClassOf rdf:resource="&java;JavaAPIPart"/>
		<rdfs:seeAlso rdf:resource="&java-se-6;JavaMath"/>
		<rdfs:seeAlso rdf:resource="&java-se-6;JavaLang"/>
		<rdfs:seeAlso rdf:resource="&java-se-6;JavaSecurity"/>
		<rdfs:seeAlso rdf:resource="&java-se-6;JavaUtil"/>
		<rdfs:seeAlso rdf:resource="&java-se-6;JavaIo"/>
		<rdfs:comment xml:lang="en">Java API part implementing the javax.security.cert package for Java SE 6</rdfs:comment>
	</owl:Class>
	<owl:Class rdf:about="&java-se-6;JavaxSecurityAuth">
		<owl:equivalentClass rdf:resource="&j2se-5_0;JavaxSecurityAuth"/>
		<rdfs:subClassOf rdf:resource="&java;JavaAPIPart"/>
		<rdfs:seeAlso rdf:resource="&java-se-6;JavaLang"/>
		<rdfs:seeAlso rdf:resource="&java-se-6;JavaSecurity"/>
		<rdfs:seeAlso rdf:resource="&java-se-6;JavaIo"/>
		<rdfs:seeAlso rdf:resource="&java-se-6;JavaUtil"/>
		<rdfs:comment xml:lang="en">Java API part implementing the javax.security.auth package for Java SE 6</rdfs:comment>
	</owl:Class>
	<owl:Class rdf:about="&java-se-6;JavaxSecurityAuthCallback">
		<owl:equivalentClass rdf:resource="&j2se-5_0;JavaxSecurityAuthCallback"/>
		<rdfs:subClassOf rdf:resource="&java;JavaAPIPart"/>
		<rdfs:seeAlso rdf:resource="&java-se-6;JavaLang"/>
		<rdfs:seeAlso rdf:resource="&java-se-6;JavaIo"/>
		<rdfs:seeAlso rdf:resource="&java-se-6;JavaUtil"/>
		<rdfs:comment xml:lang="en">Java API part implementing the javax.security.auth.callback package for Java SE 6</rdfs:comment>
	</owl:Class>
	<owl:Class rdf:about="&java-se-6;JavaxSecurityAuthLogin">
		<rdfs:subClassOf rdf:resource="&j2se-5_0;JavaxSecurityAuthLogin"/>
		<rdfs:seeAlso rdf:resource="&java-se-6;JavaxSecurityAuthCallback"/>
		<rdfs:seeAlso rdf:resource="&java-se-6;JavaLang"/>
		<rdfs:seeAlso rdf:resource="&java-se-6;JavaxSecurityAuth"/>
		<rdfs:seeAlso rdf:resource="&java-se-6;JavaSecurity"/>
		<rdfs:seeAlso rdf:resource="&java-se-6;JavaUtil"/>
		<rdfs:comment xml:lang="en">Java API part implementing the javax.security.auth.login package for Java SE 6</rdfs:comment>
	</owl:Class>
	<owl:Class rdf:about="&java-se-6;JavaxSecurityAuthX500">
		<rdfs:subClassOf rdf:resource="&j2se-5_0;JavaxSecurityAuthX500"/>
		<rdfs:seeAlso rdf:resource="&java-se-6;JavaLang"/>
		<rdfs:seeAlso rdf:resource="&java-se-6;JavaSecurityCert"/>
		<rdfs:seeAlso rdf:resource="&java-se-6;JavaSecurity"/>
		<rdfs:seeAlso rdf:resource="&java-se-6;JavaxSecurityAuth"/>
		<rdfs:seeAlso rdf:resource="&java-se-6;JavaUtil"/>
		<rdfs:seeAlso rdf:resource="&java-se-6;JavaIo"/>
		<rdfs:comment xml:lang="en">Java API part implementing the javax.security.auth.x500 package for Java SE 6</rdfs:comment>
	</owl:Class>
	<owl:Class rdf:about="&java-se-6;JavaxSecurityAuthKerberos">
		<owl:equivalentClass rdf:resource="&j2se-5_0;JavaxSecurityAuthKerberos"/>
		<rdfs:subClassOf rdf:resource="&java;JavaAPIPart"/>
		<rdfs:seeAlso rdf:resource="&java-se-6;JavaLang"/>
		<rdfs:seeAlso rdf:resource="&java-se-6;JavaSecurity"/>
		<rdfs:seeAlso rdf:resource="&java-se-6;JavaxSecurityAuth"/>
		<rdfs:seeAlso rdf:resource="&java-se-6;JavaUtil"/>
		<rdfs:seeAlso rdf:resource="&java-se-6;JavaIo"/>
		<rdfs:seeAlso rdf:resource="&java-se-6;JavaxCrypto"/>
		<rdfs:comment xml:lang="en">Java API part implementing the javax.security.auth.kerberos package for Java SE 6</rdfs:comment>
	</owl:Class>
	<owl:Class rdf:about="&java-se-6;JavaxSecurityAuthSpi">
		<owl:equivalentClass rdf:resource="&j2se-5_0;JavaxSecurityAuthSpi"/>
		<rdfs:subClassOf rdf:resource="&java;JavaAPIPart"/>
		<rdfs:seeAlso rdf:resource="&java-se-6;JavaxSecurityAuthCallback"/>
		<rdfs:seeAlso rdf:resource="&java-se-6;JavaxSecurityAuth"/>
		<rdfs:seeAlso rdf:resource="&java-se-6;JavaUtil"/>
		<rdfs:comment xml:lang="en">Java API part implementing the javax.security.auth.spi package for Java SE 6</rdfs:comment>
	</owl:Class>
	<owl:Class rdf:about="&java-se-6;JavaxSecuritySasl">
		<rdfs:subClassOf rdf:resource="&j2se-5_0;JavaxSecuritySasl"/>
		<rdfs:seeAlso rdf:resource="&java-se-6;JavaxSecurityAuthCallback"/>
		<rdfs:seeAlso rdf:resource="&java-se-6;JavaLang"/>
		<rdfs:seeAlso rdf:resource="&java-se-6;JavaIo"/>
		<rdfs:seeAlso rdf:resource="&java-se-6;JavaUtil"/>
		<rdfs:comment xml:lang="en">Java API part implementing the javax.security.sasl package for Java SE 6</rdfs:comment>
	</owl:Class>
	<owl:Class rdf:about="&java-se-6;JavaxAccessibility">
		<rdfs:subClassOf rdf:resource="&j2se-5_0;JavaxAccessibility"/>
		<rdfs:seeAlso rdf:resource="&java-se-6;JavaAwtEvent"/>
		<rdfs:seeAlso rdf:resource="&java-se-6;JavaxSwingText"/>
		<rdfs:seeAlso rdf:resource="&java-se-6;JavaAwtDatatransfer"/>
		<rdfs:seeAlso rdf:resource="&java-se-6;JavaAwt"/>
		<rdfs:seeAlso rdf:resource="&java-se-6;JavaLang"/>
		<rdfs:seeAlso rdf:resource="&java-se-6;JavaIo"/>
		<rdfs:seeAlso rdf:resource="&java-se-6;JavaBeans"/>
		<rdfs:seeAlso rdf:resource="&java-se-6;JavaUtil"/>
		<rdfs:comment xml:lang="en">Java API part implementing the javax.accessibility package for Java SE 6</rdfs:comment>
	</owl:Class>
	<owl:Class rdf:about="&java-se-6;JavaxSwing">
		<rdfs:subClassOf rdf:resource="&j2se-5_0;JavaxSwing"/>
		<rdfs:seeAlso rdf:resource="&java-se-6;JavaxSwingFilechooser"/>
		<rdfs:seeAlso rdf:resource="&java-se-6;JavaxPrint"/>
		<rdfs:seeAlso rdf:resource="&java-se-6;JavaxSwingEvent"/>
		<rdfs:seeAlso rdf:resource="&java-se-6;JavaLang"/>
		<rdfs:seeAlso rdf:resource="&java-se-6;JavaIo"/>
		<rdfs:seeAlso rdf:resource="&java-se-6;JavaUtil"/>
		<rdfs:seeAlso rdf:resource="&java-se-6;JavaxSwingPlaf"/>
		<rdfs:seeAlso rdf:resource="&java-se-6;JavaText"/>
		<rdfs:seeAlso rdf:resource="&java-se-6;JavaxSwingColorchooser"/>
		<rdfs:seeAlso rdf:resource="&java-se-6;JavaxPrintAttribute"/>
		<rdfs:seeAlso rdf:resource="&java-se-6;JavaxSwingBorder"/>
		<rdfs:seeAlso rdf:resource="&java-se-6;JavaAwtImage"/>
		<rdfs:seeAlso rdf:resource="&java-se-6;JavaBeans"/>
		<rdfs:seeAlso rdf:resource="&java-se-6;JavaAwtPrint"/>
		<rdfs:seeAlso rdf:resource="&java-se-6;JavaAwtDatatransfer"/>
		<rdfs:seeAlso rdf:resource="&java-se-6;JavaAwt"/>
		<rdfs:seeAlso rdf:resource="&java-se-6;JavaxAccessibility"/>
		<rdfs:seeAlso rdf:resource="&java-se-6;JavaxSwingTree"/>
		<rdfs:seeAlso rdf:resource="&java-se-6;JavaUtilConcurrent"/>
		<rdfs:seeAlso rdf:resource="&java-se-6;JavaxSwingText"/>
		<rdfs:seeAlso rdf:resource="&java-se-6;JavaNet"/>
		<rdfs:seeAlso rdf:resource="&java-se-6;JavaAwtEvent"/>
		<rdfs:seeAlso rdf:resource="&java-se-6;JavaApplet"/>
		<rdfs:seeAlso rdf:resource="&java-se-6;JavaxSwingTable"/>
		<rdfs:comment xml:lang="en">Java API part implementing the javax.swing package for Java SE 6</rdfs:comment>
	</owl:Class>
	<owl:Class rdf:about="&java-se-6;JavaxSwingText">
		<rdfs:subClassOf rdf:resource="&j2se-5_0;JavaxSwingText"/>
		<rdfs:seeAlso rdf:resource="&java-se-6;JavaText"/>
		<rdfs:seeAlso rdf:resource="&java-se-6;JavaxPrint"/>
		<rdfs:seeAlso rdf:resource="&java-se-6;JavaAwt"/>
		<rdfs:seeAlso rdf:resource="&java-se-6;JavaAwtIm"/>
		<rdfs:seeAlso rdf:resource="&java-se-6;JavaxSwingEvent"/>
		<rdfs:seeAlso rdf:resource="&java-se-6;JavaxSwingUndo"/>
		<rdfs:seeAlso rdf:resource="&java-se-6;JavaxSwingPlafBasic"/>
		<rdfs:seeAlso rdf:resource="&java-se-6;JavaxPrintAttribute"/>
		<rdfs:seeAlso rdf:resource="&java-se-6;JavaLang"/>
		<rdfs:seeAlso rdf:resource="&java-se-6;JavaIo"/>
		<rdfs:seeAlso rdf:resource="&java-se-6;JavaUtil"/>
		<rdfs:seeAlso rdf:resource="&java-se-6;JavaAwtEvent"/>
		<rdfs:seeAlso rdf:resource="&java-se-6;JavaxSwingPlaf"/>
		<rdfs:seeAlso rdf:resource="&java-se-6;JavaAwtPrint"/>
		<rdfs:seeAlso rdf:resource="&java-se-6;JavaxAccessibility"/>
		<rdfs:seeAlso rdf:resource="&java-se-6;JavaxSwingTree"/>
		<rdfs:seeAlso rdf:resource="&java-se-6;JavaxSwing"/>
		<rdfs:comment xml:lang="en">Java API part implementing the javax.swing.text package for Java SE 6</rdfs:comment>
	</owl:Class>
	<owl:Class rdf:about="&java-se-6;JavaxSwingTextHtml">
		<rdfs:subClassOf rdf:resource="&j2se-5_0;JavaxSwingTextHtml"/>
		<rdfs:seeAlso rdf:resource="&java-se-6;JavaxSwingText"/>
		<rdfs:seeAlso rdf:resource="&java-se-6;JavaAwt"/>
		<rdfs:seeAlso rdf:resource="&java-se-6;JavaNet"/>
		<rdfs:seeAlso rdf:resource="&java-se-6;JavaxSwingEvent"/>
		<rdfs:seeAlso rdf:resource="&java-se-6;JavaLang"/>
		<rdfs:seeAlso rdf:resource="&java-se-6;JavaIo"/>
		<rdfs:seeAlso rdf:resource="&java-se-6;JavaUtil"/>
		<rdfs:seeAlso rdf:resource="&java-se-6;JavaAwtEvent"/>
		<rdfs:seeAlso rdf:resource="&java-se-6;JavaxAccessibility"/>
		<rdfs:seeAlso rdf:resource="&java-se-6;JavaxSwing"/>
		<rdfs:comment xml:lang="en">Java API part implementing the javax.swing.text.html package for Java SE 6</rdfs:comment>
	</owl:Class>
	<owl:Class rdf:about="&java-se-6;JavaxSwingTextHtmlParser">
		<owl:equivalentClass rdf:resource="&j2se-5_0;JavaxSwingTextHtmlParser"/>
		<rdfs:subClassOf rdf:resource="&java;JavaAPIPart"/>
		<rdfs:seeAlso rdf:resource="&java-se-6;JavaxSwingText"/>
		<rdfs:seeAlso rdf:resource="&java-se-6;JavaLang"/>
		<rdfs:seeAlso rdf:resource="&java-se-6;JavaIo"/>
		<rdfs:seeAlso rdf:resource="&java-se-6;JavaUtil"/>
		<rdfs:seeAlso rdf:resource="&java-se-6;JavaxSwingTextHtml"/>
		<rdfs:comment xml:lang="en">Java API part implementing the javax.swing.text.html.parser package for Java SE 6</rdfs:comment>
	</owl:Class>
	<owl:Class rdf:about="&java-se-6;JavaxSwingTextRtf">
		<rdfs:subClassOf rdf:resource="&j2se-5_0;JavaxSwingTextRtf"/>
		<rdfs:seeAlso rdf:resource="&java-se-6;JavaxSwingText"/>
		<rdfs:seeAlso rdf:resource="&java-se-6;JavaLang"/>
		<rdfs:seeAlso rdf:resource="&java-se-6;JavaIo"/>
		<rdfs:comment xml:lang="en">Java API part implementing the javax.swing.text.rtf package for Java SE 6</rdfs:comment>
	</owl:Class>
	<owl:Class rdf:about="&java-se-6;JavaxSwingEvent">
		<rdfs:subClassOf rdf:resource="&j2se-5_0;JavaxSwingEvent"/>
		<rdfs:seeAlso rdf:resource="&java-se-6;JavaxSwingUndo"/>
		<rdfs:seeAlso rdf:resource="&java-se-6;JavaLang"/>
		<rdfs:seeAlso rdf:resource="&java-se-6;JavaIo"/>
		<rdfs:seeAlso rdf:resource="&java-se-6;JavaBeans"/>
		<rdfs:seeAlso rdf:resource="&java-se-6;JavaUtil"/>
		<rdfs:seeAlso rdf:resource="&java-se-6;JavaAwtEvent"/>
		<rdfs:seeAlso rdf:resource="&java-se-6;JavaxSwingText"/>
		<rdfs:seeAlso rdf:resource="&java-se-6;JavaxSwingTable"/>
		<rdfs:seeAlso rdf:resource="&java-se-6;JavaAwt"/>
		<rdfs:seeAlso rdf:resource="&java-se-6;JavaxSwingTree"/>
		<rdfs:seeAlso rdf:resource="&java-se-6;JavaNet"/>
		<rdfs:seeAlso rdf:resource="&java-se-6;JavaxSwing"/>
		<rdfs:comment xml:lang="en">Java API part implementing the javax.swing.event package for Java SE 6</rdfs:comment>
	</owl:Class>
	<owl:Class rdf:about="&java-se-6;JavaxSwingColorchooser">
		<rdfs:subClassOf rdf:resource="&j2se-5_0;JavaxSwingColorchooser"/>
		<rdfs:seeAlso rdf:resource="&java-se-6;JavaxSwingEvent"/>
		<rdfs:seeAlso rdf:resource="&java-se-6;JavaAwt"/>
		<rdfs:seeAlso rdf:resource="&java-se-6;JavaLang"/>
		<rdfs:seeAlso rdf:resource="&java-se-6;JavaIo"/>
		<rdfs:seeAlso rdf:resource="&java-se-6;JavaxSwing"/>
		<rdfs:comment xml:lang="en">Java API part implementing the javax.swing.colorchooser package for Java SE 6</rdfs:comment>
	</owl:Class>
	<owl:Class rdf:about="&java-se-6;JavaxSwingPlaf">
		<rdfs:subClassOf rdf:resource="&j2se-5_0;JavaxSwingPlaf"/>
		<rdfs:seeAlso rdf:resource="&java-se-6;JavaLang"/>
		<rdfs:seeAlso rdf:resource="&java-se-6;JavaxSwingFilechooser"/>
		<rdfs:seeAlso rdf:resource="&java-se-6;JavaIo"/>
		<rdfs:seeAlso rdf:resource="&java-se-6;JavaxSwingBorder"/>
		<rdfs:seeAlso rdf:resource="&java-se-6;JavaAwtEvent"/>
		<rdfs:seeAlso rdf:resource="&java-se-6;JavaxSwingText"/>
		<rdfs:seeAlso rdf:resource="&java-se-6;JavaAwt"/>
		<rdfs:seeAlso rdf:resource="&java-se-6;JavaxAccessibility"/>
		<rdfs:seeAlso rdf:resource="&java-se-6;JavaxSwingTree"/>
		<rdfs:seeAlso rdf:resource="&java-se-6;JavaxSwing"/>
		<rdfs:comment xml:lang="en">Java API part implementing the javax.swing.plaf package for Java SE 6</rdfs:comment>
	</owl:Class>
	<owl:Class rdf:about="&java-se-6;JavaxSwingPlafBasic">
		<rdfs:subClassOf rdf:resource="&j2se-5_0;JavaxSwingPlafBasic"/>
		<rdfs:seeAlso rdf:resource="&java-se-6;JavaxSwingFilechooser"/>
		<rdfs:seeAlso rdf:resource="&java-se-6;JavaAwt"/>
		<rdfs:seeAlso rdf:resource="&java-se-6;JavaxSwingEvent"/>
		<rdfs:seeAlso rdf:resource="&java-se-6;JavaLang"/>
		<rdfs:seeAlso rdf:resource="&java-se-6;JavaIo"/>
		<rdfs:seeAlso rdf:resource="&java-se-6;JavaUtil"/>
		<rdfs:seeAlso rdf:resource="&java-se-6;JavaxSwingPlaf"/>
		<rdfs:seeAlso rdf:resource="&java-se-6;JavaxAccessibility"/>
		<rdfs:seeAlso rdf:resource="&java-se-6;JavaxSwingTree"/>
		<rdfs:seeAlso rdf:resource="&java-se-6;JavaxSwingText"/>
		<rdfs:seeAlso rdf:resource="&java-se-6;JavaxSwingBorder"/>
		<rdfs:seeAlso rdf:resource="&java-se-6;JavaBeans"/>
		<rdfs:seeAlso rdf:resource="&java-se-6;JavaAwtEvent"/>
		<rdfs:seeAlso rdf:resource="&java-se-6;JavaxSwingTable"/>
		<rdfs:seeAlso rdf:resource="&java-se-6;JavaxSwing"/>
		<rdfs:comment xml:lang="en">Java API part implementing the javax.swing.plaf.basic package for Java SE 6</rdfs:comment>
	</owl:Class>
	<owl:Class rdf:about="&java-se-6;JavaxSwingPlafMetal">
		<rdfs:subClassOf rdf:resource="&j2se-5_0;JavaxSwingPlafMetal"/>
		<rdfs:seeAlso rdf:resource="&java-se-6;JavaAwt"/>
		<rdfs:seeAlso rdf:resource="&java-se-6;JavaxSwingEvent"/>
		<rdfs:seeAlso rdf:resource="&java-se-6;JavaLang"/>
		<rdfs:seeAlso rdf:resource="&java-se-6;JavaxSwingPlafBasic"/>
		<rdfs:seeAlso rdf:resource="&java-se-6;JavaIo"/>
		<rdfs:seeAlso rdf:resource="&java-se-6;JavaxSwingBorder"/>
		<rdfs:seeAlso rdf:resource="&java-se-6;JavaBeans"/>
		<rdfs:seeAlso rdf:resource="&java-se-6;JavaAwtEvent"/>
		<rdfs:seeAlso rdf:resource="&java-se-6;JavaxSwingPlaf"/>
		<rdfs:seeAlso rdf:resource="&java-se-6;JavaxSwingTree"/>
		<rdfs:seeAlso rdf:resource="&java-se-6;JavaxSwing"/>
		<rdfs:comment xml:lang="en">Java API part implementing the javax.swing.plaf.metal package for Java SE 6</rdfs:comment>
	</owl:Class>
	<owl:Class rdf:about="&java-se-6;JavaxSwingPlafMulti">
		<rdfs:subClassOf rdf:resource="&j2se-5_0;JavaxSwingPlafMulti"/>
		<rdfs:seeAlso rdf:resource="&java-se-6;JavaxSwingFilechooser"/>
		<rdfs:seeAlso rdf:resource="&java-se-6;JavaxSwingText"/>
		<rdfs:seeAlso rdf:resource="&java-se-6;JavaAwt"/>
		<rdfs:seeAlso rdf:resource="&java-se-6;JavaLang"/>
		<rdfs:seeAlso rdf:resource="&java-se-6;JavaIo"/>
		<rdfs:seeAlso rdf:resource="&java-se-6;JavaUtil"/>
		<rdfs:seeAlso rdf:resource="&java-se-6;JavaAwtEvent"/>
		<rdfs:seeAlso rdf:resource="&java-se-6;JavaxSwingPlaf"/>
		<rdfs:seeAlso rdf:resource="&java-se-6;JavaxAccessibility"/>
		<rdfs:seeAlso rdf:resource="&java-se-6;JavaxSwingTree"/>
		<rdfs:seeAlso rdf:resource="&java-se-6;JavaxSwing"/>
		<rdfs:comment xml:lang="en">Java API part implementing the javax.swing.plaf.multi package for Java SE 6</rdfs:comment>
	</owl:Class>
	<owl:Class rdf:about="&java-se-6;JavaxSwingPlafSynth">
		<rdfs:subClassOf rdf:resource="&j2se-5_0;JavaxSwingPlafSynth"/>
		<rdfs:seeAlso rdf:resource="&java-se-6;JavaAwtEvent"/>
		<rdfs:seeAlso rdf:resource="&java-se-6;JavaAwt"/>
		<rdfs:seeAlso rdf:resource="&java-se-6;JavaLang"/>
		<rdfs:seeAlso rdf:resource="&java-se-6;JavaxSwingPlafBasic"/>
		<rdfs:seeAlso rdf:resource="&java-se-6;JavaxSwingPlaf"/>
		<rdfs:seeAlso rdf:resource="&java-se-6;JavaIo"/>
		<rdfs:seeAlso rdf:resource="&java-se-6;JavaNet"/>
		<rdfs:seeAlso rdf:resource="&java-se-6;JavaxSwing"/>
		<rdfs:comment xml:lang="en">Java API part implementing the javax.swing.plaf.synth package for Java SE 6</rdfs:comment>
	</owl:Class>
	<owl:Class rdf:about="&java-se-6;JavaxSwingFilechooser">
		<rdfs:subClassOf rdf:resource="&j2se-5_0;JavaxSwingFilechooser"/>
		<rdfs:seeAlso rdf:resource="&java-se-6;JavaxSwing"/>
		<rdfs:seeAlso rdf:resource="&java-se-6;JavaLang"/>
		<rdfs:seeAlso rdf:resource="&java-se-6;JavaIo"/>
		<rdfs:comment xml:lang="en">Java API part implementing the javax.swing.filechooser package for Java SE 6</rdfs:comment>
	</owl:Class>
	<owl:Class rdf:about="&java-se-6;JavaxSwingTree">
		<rdfs:subClassOf rdf:resource="&j2se-5_0;JavaxSwingTree"/>
		<rdfs:seeAlso rdf:resource="&java-se-6;JavaxSwingEvent"/>
		<rdfs:seeAlso rdf:resource="&java-se-6;JavaLang"/>
		<rdfs:seeAlso rdf:resource="&java-se-6;JavaIo"/>
		<rdfs:seeAlso rdf:resource="&java-se-6;JavaxSwingBorder"/>
		<rdfs:seeAlso rdf:resource="&java-se-6;JavaBeans"/>
		<rdfs:seeAlso rdf:resource="&java-se-6;JavaUtil"/>
		<rdfs:seeAlso rdf:resource="&java-se-6;JavaAwtEvent"/>
		<rdfs:seeAlso rdf:resource="&java-se-6;JavaAwt"/>
		<rdfs:seeAlso rdf:resource="&java-se-6;JavaxSwing"/>
		<rdfs:comment xml:lang="en">Java API part implementing the javax.swing.tree package for Java SE 6</rdfs:comment>
	</owl:Class>
	<owl:Class rdf:about="&java-se-6;JavaxSwingBorder">
		<rdfs:subClassOf rdf:resource="&j2se-5_0;JavaxSwingBorder"/>
		<rdfs:seeAlso rdf:resource="&java-se-6;JavaAwt"/>
		<rdfs:seeAlso rdf:resource="&java-se-6;JavaLang"/>
		<rdfs:seeAlso rdf:resource="&java-se-6;JavaIo"/>
		<rdfs:seeAlso rdf:resource="&java-se-6;JavaxSwing"/>
		<rdfs:comment xml:lang="en">Java API part implementing the javax.swing.border package for Java SE 6</rdfs:comment>
	</owl:Class>
	<owl:Class rdf:about="&java-se-6;JavaxSwingTable">
		<rdfs:subClassOf rdf:resource="&j2se-5_0;JavaxSwingTable"/>
		<rdfs:seeAlso rdf:resource="&java-se-6;JavaxSwingEvent"/>
		<rdfs:seeAlso rdf:resource="&java-se-6;JavaLang"/>
		<rdfs:seeAlso rdf:resource="&java-se-6;JavaIo"/>
		<rdfs:seeAlso rdf:resource="&java-se-6;JavaxSwingBorder"/>
		<rdfs:seeAlso rdf:resource="&java-se-6;JavaBeans"/>
		<rdfs:seeAlso rdf:resource="&java-se-6;JavaUtil"/>
		<rdfs:seeAlso rdf:resource="&java-se-6;JavaAwtEvent"/>
		<rdfs:seeAlso rdf:resource="&java-se-6;JavaAwt"/>
		<rdfs:seeAlso rdf:resource="&java-se-6;JavaxSwingPlaf"/>
		<rdfs:seeAlso rdf:resource="&java-se-6;JavaxAccessibility"/>
		<rdfs:seeAlso rdf:resource="&java-se-6;JavaxSwing"/>
		<rdfs:comment xml:lang="en">Java API part implementing the javax.swing.table package for Java SE 6</rdfs:comment>
	</owl:Class>
	<owl:Class rdf:about="&java-se-6;JavaxSwingUndo">
		<owl:equivalentClass rdf:resource="&j2se-5_0;JavaxSwingUndo"/>
		<rdfs:subClassOf rdf:resource="&java;JavaAPIPart"/>
		<rdfs:seeAlso rdf:resource="&java-se-6;JavaxSwingEvent"/>
		<rdfs:seeAlso rdf:resource="&java-se-6;JavaLang"/>
		<rdfs:seeAlso rdf:resource="&java-se-6;JavaIo"/>
		<rdfs:seeAlso rdf:resource="&java-se-6;JavaUtil"/>
		<rdfs:comment xml:lang="en">Java API part implementing the javax.swing.undo package for Java SE 6</rdfs:comment>
	</owl:Class>
	<owl:Class rdf:about="&java-se-6;JavaxManagement">
		<rdfs:subClassOf rdf:resource="&j2se-5_0;JavaxManagement"/>
		<rdfs:seeAlso rdf:resource="&java-se-6;JavaUtilConcurrent"/>
		<rdfs:seeAlso rdf:resource="&java-se-6;JavaLang"/>
		<rdfs:seeAlso rdf:resource="&java-se-6;JavaxManagementLoading"/>
		<rdfs:seeAlso rdf:resource="&java-se-6;JavaIo"/>
		<rdfs:seeAlso rdf:resource="&java-se-6;JavaUtil"/>
		<rdfs:seeAlso rdf:resource="&java-se-6;JavaSecurity"/>
		<rdfs:seeAlso rdf:resource="&java-se-6;JavaLangReflect"/>
		<rdfs:seeAlso rdf:resource="&java-se-6;JavaLangAnnotation"/>
		<rdfs:comment xml:lang="en">Java API part implementing the javax.management package for Java SE 6</rdfs:comment>
	</owl:Class>
	<owl:Class rdf:about="&java-se-6;JavaxManagementOpenmbean">
		<rdfs:subClassOf rdf:resource="&j2se-5_0;JavaxManagementOpenmbean"/>
		<rdfs:seeAlso rdf:resource="&java-se-6;JavaxManagement"/>
		<rdfs:seeAlso rdf:resource="&java-se-6;JavaLang"/>
		<rdfs:seeAlso rdf:resource="&java-se-6;JavaIo"/>
		<rdfs:seeAlso rdf:resource="&java-se-6;JavaLangReflect"/>
		<rdfs:seeAlso rdf:resource="&java-se-6;JavaUtil"/>
		<rdfs:comment xml:lang="en">Java API part implementing the javax.management.openmbean package for Java SE 6</rdfs:comment>
	</owl:Class>
	<owl:Class rdf:about="&java-se-6;JavaxManagementLoading">
		<rdfs:subClassOf rdf:resource="&j2se-5_0;JavaxManagementLoading"/>
		<rdfs:seeAlso rdf:resource="&java-se-6;JavaxManagement"/>
		<rdfs:seeAlso rdf:resource="&java-se-6;JavaLang"/>
		<rdfs:seeAlso rdf:resource="&java-se-6;JavaIo"/>
		<rdfs:seeAlso rdf:resource="&java-se-6;JavaNet"/>
		<rdfs:seeAlso rdf:resource="&java-se-6;JavaUtil"/>
		<rdfs:comment xml:lang="en">Java API part implementing the javax.management.loading package for Java SE 6</rdfs:comment>
	</owl:Class>
	<owl:Class rdf:about="&java-se-6;JavaxManagementModelmbean">
		<rdfs:subClassOf rdf:resource="&j2se-5_0;JavaxManagementModelmbean"/>
		<rdfs:seeAlso rdf:resource="&java-se-6;JavaLang"/>
		<rdfs:seeAlso rdf:resource="&java-se-6;JavaxManagementLoading"/>
		<rdfs:seeAlso rdf:resource="&java-se-6;JavaxManagement"/>
		<rdfs:seeAlso rdf:resource="&java-se-6;JavaLangReflect"/>
		<rdfs:comment xml:lang="en">Java API part implementing the javax.management.modelmbean package for Java SE 6</rdfs:comment>
	</owl:Class>
	<owl:Class rdf:about="&java-se-6;JavaxManagementMonitor">
		<rdfs:subClassOf rdf:resource="&j2se-5_0;JavaxManagementMonitor"/>
		<rdfs:seeAlso rdf:resource="&java-se-6;JavaLang"/>
		<rdfs:seeAlso rdf:resource="&java-se-6;JavaxManagement"/>
		<rdfs:comment xml:lang="en">Java API part implementing the javax.management.monitor package for Java SE 6</rdfs:comment>
	</owl:Class>
	<owl:Class rdf:about="&java-se-6;JavaxManagementRelation">
		<rdfs:subClassOf rdf:resource="&j2se-5_0;JavaxManagementRelation"/>
		<rdfs:seeAlso rdf:resource="&java-se-6;JavaLang"/>
		<rdfs:seeAlso rdf:resource="&java-se-6;JavaxManagement"/>
		<rdfs:seeAlso rdf:resource="&java-se-6;JavaIo"/>
		<rdfs:seeAlso rdf:resource="&java-se-6;JavaUtil"/>
		<rdfs:comment xml:lang="en">Java API part implementing the javax.management.relation package for Java SE 6</rdfs:comment>
	</owl:Class>
	<owl:Class rdf:about="&java-se-6;JavaxManagementRemote">
		<rdfs:subClassOf rdf:resource="&j2se-5_0;JavaxManagementRemote"/>
		<rdfs:seeAlso rdf:resource="&java-se-6;JavaxManagement"/>
		<rdfs:seeAlso rdf:resource="&java-se-6;JavaLang"/>
		<rdfs:seeAlso rdf:resource="&java-se-6;JavaSecurity"/>
		<rdfs:seeAlso rdf:resource="&java-se-6;JavaIo"/>
		<rdfs:seeAlso rdf:resource="&java-se-6;JavaxSecurityAuth"/>
		<rdfs:seeAlso rdf:resource="&java-se-6;JavaUtil"/>
		<rdfs:comment xml:lang="en">Java API part implementing the javax.management.remote package for Java SE 6</rdfs:comment>
	</owl:Class>
	<owl:Class rdf:about="&java-se-6;JavaxManagementRemoteRmi">
		<rdfs:subClassOf rdf:resource="&j2se-5_0;JavaxManagementRemoteRmi"/>
		<rdfs:seeAlso rdf:resource="&java-se-6;OrgOmgCORBAPortable"/>
		<rdfs:seeAlso rdf:resource="&java-se-6;JavaLang"/>
		<rdfs:seeAlso rdf:resource="&java-se-6;JavaIo"/>
		<rdfs:seeAlso rdf:resource="&java-se-6;JavaRmi"/>
		<rdfs:seeAlso rdf:resource="&java-se-6;OrgOmgCORBA_2_3Portable"/>
		<rdfs:seeAlso rdf:resource="&java-se-6;JavaxManagementRemote"/>
		<rdfs:seeAlso rdf:resource="&java-se-6;OrgOmgCORBA"/>
		<rdfs:seeAlso rdf:resource="&java-se-6;JavaxRmiCORBA"/>
		<rdfs:seeAlso rdf:resource="&java-se-6;JavaxSecurityAuth"/>
		<rdfs:seeAlso rdf:resource="&java-se-6;JavaUtil"/>
		<rdfs:seeAlso rdf:resource="&java-se-6;JavaRmiServer"/>
		<rdfs:seeAlso rdf:resource="&java-se-6;JavaxManagement"/>
		<rdfs:comment xml:lang="en">Java API part implementing the javax.management.remote.rmi package for Java SE 6</rdfs:comment>
	</owl:Class>
	<owl:Class rdf:about="&java-se-6;JavaxManagementTimer">
		<rdfs:subClassOf rdf:resource="&java;JavaAPIPart"/>
		<rdfs:seeAlso rdf:resource="&java-se-6;JavaLang"/>
		<rdfs:seeAlso rdf:resource="&java-se-6;JavaxManagement"/>
		<rdfs:seeAlso rdf:resource="&java-se-6;JavaUtil"/>
		<rdfs:comment xml:lang="en">Java API part implementing the javax.management.timer package for Java SE 6</rdfs:comment>
	</owl:Class>
	<owl:Class rdf:about="&java-se-6;JavaxXml">
		<owl:equivalentClass rdf:resource="&j2se-5_0;JavaxXml"/>
		<rdfs:subClassOf rdf:resource="&java;JavaAPIPart"/>
		<rdfs:seeAlso rdf:resource="&java-se-6;JavaLang"/>
		<rdfs:comment xml:lang="en">Java API part implementing the javax.xml package for Java SE 6</rdfs:comment>
	</owl:Class>
	<owl:Class rdf:about="&java-se-6;JavaxXmlTransform">
		<rdfs:subClassOf rdf:resource="&j2se-5_0;JavaxXmlTransform"/>
		<rdfs:seeAlso rdf:resource="&java-se-6;JavaLang"/>
		<rdfs:seeAlso rdf:resource="&java-se-6;JavaIo"/>
		<rdfs:seeAlso rdf:resource="&java-se-6;JavaUtil"/>
		<rdfs:comment xml:lang="en">Java API part implementing the javax.xml.transform package for Java SE 6</rdfs:comment>
	</owl:Class>
	<owl:Class rdf:about="&java-se-6;JavaxXmlTransformDom">
		<owl:equivalentClass rdf:resource="&j2se-5_0;JavaxXmlTransformDom"/>
		<rdfs:subClassOf rdf:resource="&java;JavaAPIPart"/>
		<rdfs:seeAlso rdf:resource="&java-se-6;JavaxXmlTransform"/>
		<rdfs:seeAlso rdf:resource="&java-se-6;OrgW3cDom"/>
		<rdfs:seeAlso rdf:resource="&java-se-6;JavaLang"/>
		<rdfs:comment xml:lang="en">Java API part implementing the javax.xml.transform.dom package for Java SE 6</rdfs:comment>
	</owl:Class>
	<owl:Class rdf:about="&java-se-6;JavaxXmlTransformSax">
		<rdfs:subClassOf rdf:resource="&j2se-5_0;JavaxXmlTransformSax"/>
		<rdfs:seeAlso rdf:resource="&java-se-6;JavaxXmlTransform"/>
		<rdfs:seeAlso rdf:resource="&java-se-6;JavaLang"/>
		<rdfs:seeAlso rdf:resource="&java-se-6;OrgXmlSax"/>
		<rdfs:seeAlso rdf:resource="&java-se-6;OrgXmlSaxExt"/>
		<rdfs:comment xml:lang="en">Java API part implementing the javax.xml.transform.sax package for Java SE 6</rdfs:comment>
	</owl:Class>
	<owl:Class rdf:about="&java-se-6;JavaxXmlTransformStax">
		<rdfs:subClassOf rdf:resource="&java;JavaAPIPart"/>
		<rdfs:seeAlso rdf:resource="&java-se-6;JavaxXmlTransform"/>
		<rdfs:seeAlso rdf:resource="&java-se-6;JavaxXmlStream"/>
		<rdfs:seeAlso rdf:resource="&java-se-6;JavaLang"/>
		<rdfs:comment xml:lang="en">Java API part implementing the javax.xml.transform.stax package for Java SE 6</rdfs:comment>
	</owl:Class>
	<owl:Class rdf:about="&java-se-6;JavaxXmlTransformStream">
		<owl:equivalentClass rdf:resource="&j2se-5_0;JavaxXmlTransformStream"/>
		<rdfs:subClassOf rdf:resource="&java;JavaAPIPart"/>
		<rdfs:seeAlso rdf:resource="&java-se-6;JavaxXmlTransform"/>
		<rdfs:seeAlso rdf:resource="&java-se-6;JavaLang"/>
		<rdfs:seeAlso rdf:resource="&java-se-6;JavaIo"/>
		<rdfs:comment xml:lang="en">Java API part implementing the javax.xml.transform.stream package for Java SE 6</rdfs:comment>
	</owl:Class>
	<owl:Class rdf:about="&java-se-6;JavaxXmlBind">
		<rdfs:subClassOf rdf:resource="&java;JavaAPIPart"/>
		<rdfs:seeAlso rdf:resource="&java-se-6;JavaLang"/>
		<rdfs:seeAlso rdf:resource="&java-se-6;JavaxXmlBindAttachment"/>
		<rdfs:seeAlso rdf:resource="&java-se-6;JavaIo"/>
		<rdfs:seeAlso rdf:resource="&java-se-6;JavaxXmlValidation"/>
		<rdfs:seeAlso rdf:resource="&java-se-6;JavaUtil"/>
		<rdfs:seeAlso rdf:resource="&java-se-6;JavaxXmlTransform"/>
		<rdfs:seeAlso rdf:resource="&java-se-6;OrgW3cDom"/>
		<rdfs:seeAlso rdf:resource="&java-se-6;OrgXmlSax"/>
		<rdfs:seeAlso rdf:resource="&java-se-6;JavaxXmlNamespace"/>
		<rdfs:seeAlso rdf:resource="&java-se-6;JavaxXmlStream"/>
		<rdfs:seeAlso rdf:resource="&java-se-6;JavaNet"/>
		<rdfs:seeAlso rdf:resource="&java-se-6;JavaMath"/>
		<rdfs:seeAlso rdf:resource="&java-se-6;JavaxXmlBindAnnotationAdapters"/>
		<rdfs:comment xml:lang="en">Java API part implementing the javax.xml.bind package for Java SE 6</rdfs:comment>
	</owl:Class>
	<owl:Class rdf:about="&java-se-6;JavaxXmlBindAnnotation">
		<rdfs:subClassOf rdf:resource="&java;JavaAPIPart"/>
		<rdfs:seeAlso rdf:resource="&java-se-6;JavaxXmlTransform"/>
		<rdfs:seeAlso rdf:resource="&java-se-6;JavaxXmlTransformDom"/>
		<rdfs:seeAlso rdf:resource="&java-se-6;JavaxXmlParsers"/>
		<rdfs:seeAlso rdf:resource="&java-se-6;OrgW3cDom"/>
		<rdfs:seeAlso rdf:resource="&java-se-6;JavaxXmlBind"/>
		<rdfs:seeAlso rdf:resource="&java-se-6;JavaLang"/>
		<rdfs:seeAlso rdf:resource="&java-se-6;JavaLangAnnotation"/>
		<rdfs:comment xml:lang="en">Java API part implementing the javax.xml.bind.annotation package for Java SE 6</rdfs:comment>
	</owl:Class>
	<owl:Class rdf:about="&java-se-6;JavaxXmlBindAnnotationAdapters">
		<rdfs:subClassOf rdf:resource="&java;JavaAPIPart"/>
		<rdfs:seeAlso rdf:resource="&java-se-6;JavaLang"/>
		<rdfs:seeAlso rdf:resource="&java-se-6;JavaLangAnnotation"/>
		<rdfs:comment xml:lang="en">Java API part implementing the javax.xml.bind.annotation.adapters package for Java SE 6</rdfs:comment>
	</owl:Class>
	<owl:Class rdf:about="&java-se-6;JavaxXmlBindAttachment">
		<rdfs:subClassOf rdf:resource="&java;JavaAPIPart"/>
		<rdfs:seeAlso rdf:resource="&java-se-6;JavaxActivation"/>
		<rdfs:seeAlso rdf:resource="&java-se-6;JavaLang"/>
		<rdfs:comment xml:lang="en">Java API part implementing the javax.xml.bind.attachment package for Java SE 6</rdfs:comment>
	</owl:Class>
	<owl:Class rdf:about="&java-se-6;JavaxXmlBindHelpers">
		<rdfs:subClassOf rdf:resource="&java;JavaAPIPart"/>
		<rdfs:seeAlso rdf:resource="&java-se-6;JavaLang"/>
		<rdfs:seeAlso rdf:resource="&java-se-6;JavaxXmlBindAttachment"/>
		<rdfs:seeAlso rdf:resource="&java-se-6;JavaIo"/>
		<rdfs:seeAlso rdf:resource="&java-se-6;JavaxXmlValidation"/>
		<rdfs:seeAlso rdf:resource="&java-se-6;JavaxXmlTransform"/>
		<rdfs:seeAlso rdf:resource="&java-se-6;OrgW3cDom"/>
		<rdfs:seeAlso rdf:resource="&java-se-6;JavaxXmlBind"/>
		<rdfs:seeAlso rdf:resource="&java-se-6;OrgXmlSax"/>
		<rdfs:seeAlso rdf:resource="&java-se-6;JavaxXmlStream"/>
		<rdfs:seeAlso rdf:resource="&java-se-6;JavaNet"/>
		<rdfs:seeAlso rdf:resource="&java-se-6;JavaxXmlBindAnnotationAdapters"/>
		<rdfs:comment xml:lang="en">Java API part implementing the javax.xml.bind.helpers package for Java SE 6</rdfs:comment>
	</owl:Class>
	<owl:Class rdf:about="&java-se-6;JavaxXmlBindUtil">
		<rdfs:subClassOf rdf:resource="&java;JavaAPIPart"/>
		<rdfs:seeAlso rdf:resource="&java-se-6;JavaxXmlBind"/>
		<rdfs:seeAlso rdf:resource="&java-se-6;JavaLang"/>
		<rdfs:seeAlso rdf:resource="&java-se-6;JavaxXmlTransformSax"/>
		<rdfs:comment xml:lang="en">Java API part implementing the javax.xml.bind.util package for Java SE 6</rdfs:comment>
	</owl:Class>
	<owl:Class rdf:about="&java-se-6;JavaxXmlValidation">
		<rdfs:subClassOf rdf:resource="&j2se-5_0;JavaxXmlValidation"/>
		<rdfs:seeAlso rdf:resource="&java-se-6;JavaxXmlTransform"/>
		<rdfs:seeAlso rdf:resource="&java-se-6;JavaNet"/>
		<rdfs:seeAlso rdf:resource="&java-se-6;OrgW3cDom"/>
		<rdfs:seeAlso rdf:resource="&java-se-6;JavaLang"/>
		<rdfs:seeAlso rdf:resource="&java-se-6;OrgXmlSax"/>
		<rdfs:seeAlso rdf:resource="&java-se-6;JavaIo"/>
		<rdfs:seeAlso rdf:resource="&java-se-6;OrgW3cDomLs"/>
		<rdfs:comment xml:lang="en">Java API part implementing the javax.xml.validation package for Java SE 6</rdfs:comment>
	</owl:Class>
	<owl:Class rdf:about="&java-se-6;JavaxXmlNamespace">
		<owl:equivalentClass rdf:resource="&j2se-5_0;JavaxXmlNamespace"/>
		<rdfs:subClassOf rdf:resource="&java;JavaAPIPart"/>
		<rdfs:seeAlso rdf:resource="&java-se-6;JavaLang"/>
		<rdfs:seeAlso rdf:resource="&java-se-6;JavaUtil"/>
		<rdfs:seeAlso rdf:resource="&java-se-6;JavaIo"/>
		<rdfs:comment xml:lang="en">Java API part implementing the javax.xml.namespace package for Java SE 6</rdfs:comment>
	</owl:Class>
	<owl:Class rdf:about="&java-se-6;JavaxXmlStream">
		<rdfs:subClassOf rdf:resource="&java;JavaAPIPart"/>
		<rdfs:seeAlso rdf:resource="&java-se-6;JavaxXmlStreamEvents"/>
		<rdfs:seeAlso rdf:resource="&java-se-6;JavaLang"/>
		<rdfs:seeAlso rdf:resource="&java-se-6;JavaIo"/>
		<rdfs:seeAlso rdf:resource="&java-se-6;JavaUtil"/>
		<rdfs:seeAlso rdf:resource="&java-se-6;JavaxXmlTransform"/>
		<rdfs:seeAlso rdf:resource="&java-se-6;JavaxXmlStreamUtil"/>
		<rdfs:seeAlso rdf:resource="&java-se-6;JavaxXmlNamespace"/>
		<rdfs:comment xml:lang="en">Java API part implementing the javax.xml.stream package for Java SE 6</rdfs:comment>
	</owl:Class>
	<owl:Class rdf:about="&java-se-6;JavaxXmlStreamEvents">
		<rdfs:subClassOf rdf:resource="&java;JavaAPIPart"/>
		<rdfs:seeAlso rdf:resource="&java-se-6;JavaxXmlStream"/>
		<rdfs:seeAlso rdf:resource="&java-se-6;JavaLang"/>
		<rdfs:seeAlso rdf:resource="&java-se-6;JavaUtil"/>
		<rdfs:seeAlso rdf:resource="&java-se-6;JavaIo"/>
		<rdfs:seeAlso rdf:resource="&java-se-6;JavaxXmlNamespace"/>
		<rdfs:comment xml:lang="en">Java API part implementing the javax.xml.stream.events package for Java SE 6</rdfs:comment>
	</owl:Class>
	<owl:Class rdf:about="&java-se-6;JavaxXmlStreamUtil">
		<rdfs:subClassOf rdf:resource="&java;JavaAPIPart"/>
		<rdfs:seeAlso rdf:resource="&java-se-6;JavaxXmlStreamEvents"/>
		<rdfs:seeAlso rdf:resource="&java-se-6;JavaxXmlStream"/>
		<rdfs:seeAlso rdf:resource="&java-se-6;JavaLang"/>
		<rdfs:seeAlso rdf:resource="&java-se-6;JavaxXmlNamespace"/>
		<rdfs:comment xml:lang="en">Java API part implementing the javax.xml.stream.util package for Java SE 6</rdfs:comment>
	</owl:Class>
	<owl:Class rdf:about="&java-se-6;JavaxXmlParsers">
		<rdfs:subClassOf rdf:resource="&j2se-5_0;JavaxXmlParsers"/>
		<rdfs:seeAlso rdf:resource="&java-se-6;OrgW3cDom"/>
		<rdfs:seeAlso rdf:resource="&java-se-6;JavaLang"/>
		<rdfs:seeAlso rdf:resource="&java-se-6;OrgXmlSax"/>
		<rdfs:seeAlso rdf:resource="&java-se-6;JavaIo"/>
		<rdfs:seeAlso rdf:resource="&java-se-6;OrgXmlSaxHelpers"/>
		<rdfs:seeAlso rdf:resource="&java-se-6;JavaxXmlValidation"/>
		<rdfs:comment xml:lang="en">Java API part implementing the javax.xml.parsers package for Java SE 6</rdfs:comment>
	</owl:Class>
	<owl:Class rdf:about="&java-se-6;JavaxXmlCrypto">
		<rdfs:subClassOf rdf:resource="&java;JavaAPIPart"/>
		<rdfs:seeAlso rdf:resource="&java-se-6;JavaSecuritySpec"/>
		<rdfs:seeAlso rdf:resource="&java-se-6;JavaxXmlCryptoDsigKeyinfo"/>
		<rdfs:seeAlso rdf:resource="&java-se-6;JavaLang"/>
		<rdfs:seeAlso rdf:resource="&java-se-6;JavaSecurity"/>
		<rdfs:seeAlso rdf:resource="&java-se-6;JavaIo"/>
		<rdfs:seeAlso rdf:resource="&java-se-6;JavaUtil"/>
		<rdfs:comment xml:lang="en">Java API part implementing the javax.xml.crypto package for Java SE 6</rdfs:comment>
	</owl:Class>
	<owl:Class rdf:about="&java-se-6;JavaxXmlCryptoDsig">
		<rdfs:subClassOf rdf:resource="&java;JavaAPIPart"/>
		<rdfs:seeAlso rdf:resource="&java-se-6;JavaSecuritySpec"/>
		<rdfs:seeAlso rdf:resource="&java-se-6;JavaLang"/>
		<rdfs:seeAlso rdf:resource="&java-se-6;JavaxXmlCryptoDsigKeyinfo"/>
		<rdfs:seeAlso rdf:resource="&java-se-6;JavaIo"/>
		<rdfs:seeAlso rdf:resource="&java-se-6;JavaxXmlCryptoDsigSpec"/>
		<rdfs:seeAlso rdf:resource="&java-se-6;JavaUtil"/>
		<rdfs:seeAlso rdf:resource="&java-se-6;JavaSecurity"/>
		<rdfs:seeAlso rdf:resource="&java-se-6;JavaxXmlCrypto"/>
		<rdfs:comment xml:lang="en">Java API part implementing the javax.xml.crypto.dsig package for Java SE 6</rdfs:comment>
	</owl:Class>
	<owl:Class rdf:about="&java-se-6;JavaxXmlCryptoDsigKeyinfo">
		<rdfs:subClassOf rdf:resource="&java;JavaAPIPart"/>
		<rdfs:seeAlso rdf:resource="&java-se-6;JavaMath"/>
		<rdfs:seeAlso rdf:resource="&java-se-6;JavaLang"/>
		<rdfs:seeAlso rdf:resource="&java-se-6;JavaxXmlCrypto"/>
		<rdfs:seeAlso rdf:resource="&java-se-6;JavaSecurity"/>
		<rdfs:seeAlso rdf:resource="&java-se-6;JavaUtil"/>
		<rdfs:comment xml:lang="en">Java API part implementing the javax.xml.crypto.dsig.keyinfo package for Java SE 6</rdfs:comment>
	</owl:Class>
	<owl:Class rdf:about="&java-se-6;JavaxXmlCryptoDsigSpec">
		<rdfs:subClassOf rdf:resource="&java;JavaAPIPart"/>
		<rdfs:seeAlso rdf:resource="&java-se-6;JavaSecuritySpec"/>
		<rdfs:seeAlso rdf:resource="&java-se-6;JavaLang"/>
		<rdfs:seeAlso rdf:resource="&java-se-6;JavaxXmlCrypto"/>
		<rdfs:seeAlso rdf:resource="&java-se-6;JavaUtil"/>
		<rdfs:comment xml:lang="en">Java API part implementing the javax.xml.crypto.dsig.spec package for Java SE 6</rdfs:comment>
	</owl:Class>
	<owl:Class rdf:about="&java-se-6;JavaxXmlCryptoDsigDom">
		<rdfs:subClassOf rdf:resource="&java;JavaAPIPart"/>
		<rdfs:seeAlso rdf:resource="&java-se-6;JavaxXmlCryptoDsig"/>
		<rdfs:seeAlso rdf:resource="&java-se-6;OrgW3cDom"/>
		<rdfs:seeAlso rdf:resource="&java-se-6;JavaxXmlCryptoDom"/>
		<rdfs:seeAlso rdf:resource="&java-se-6;JavaSecurity"/>
		<rdfs:seeAlso rdf:resource="&java-se-6;JavaxXmlCrypto"/>
		<rdfs:comment xml:lang="en">Java API part implementing the javax.xml.crypto.dsig.dom package for Java SE 6</rdfs:comment>
	</owl:Class>
	<owl:Class rdf:about="&java-se-6;JavaxXmlCryptoDom">
		<rdfs:subClassOf rdf:resource="&java;JavaAPIPart"/>
		<rdfs:seeAlso rdf:resource="&java-se-6;OrgW3cDom"/>
		<rdfs:seeAlso rdf:resource="&java-se-6;JavaLang"/>
		<rdfs:seeAlso rdf:resource="&java-se-6;JavaxXmlCrypto"/>
		<rdfs:seeAlso rdf:resource="&java-se-6;JavaUtil"/>
		<rdfs:comment xml:lang="en">Java API part implementing the javax.xml.crypto.dom package for Java SE 6</rdfs:comment>
	</owl:Class>
	<owl:Class rdf:about="&java-se-6;JavaxXmlDatatype">
		<rdfs:subClassOf rdf:resource="&j2se-5_0;JavaxXmlDatatype"/>
		<rdfs:seeAlso rdf:resource="&java-se-6;JavaLang"/>
		<rdfs:seeAlso rdf:resource="&java-se-6;JavaxXmlNamespace"/>
		<rdfs:seeAlso rdf:resource="&java-se-6;JavaMath"/>
		<rdfs:seeAlso rdf:resource="&java-se-6;JavaUtil"/>
		<rdfs:comment xml:lang="en">Java API part implementing the javax.xml.datatype package for Java SE 6</rdfs:comment>
	</owl:Class>
	<owl:Class rdf:about="&java-se-6;JavaxXmlSoap">
		<rdfs:subClassOf rdf:resource="&java;JavaAPIPart"/>
		<rdfs:seeAlso rdf:resource="&java-se-6;JavaxXmlTransform"/>
		<rdfs:seeAlso rdf:resource="&java-se-6;OrgW3cDom"/>
		<rdfs:seeAlso rdf:resource="&java-se-6;JavaLang"/>
		<rdfs:seeAlso rdf:resource="&java-se-6;JavaIo"/>
		<rdfs:seeAlso rdf:resource="&java-se-6;JavaxXmlNamespace"/>
		<rdfs:seeAlso rdf:resource="&java-se-6;JavaxXmlTransformDom"/>
		<rdfs:seeAlso rdf:resource="&java-se-6;JavaxActivation"/>
		<rdfs:seeAlso rdf:resource="&java-se-6;JavaUtil"/>
		<rdfs:comment xml:lang="en">Java API part implementing the javax.xml.soap package for Java SE 6</rdfs:comment>
	</owl:Class>
	<owl:Class rdf:about="&java-se-6;JavaxXmlWs">
		<rdfs:subClassOf rdf:resource="&java;JavaAPIPart"/>
		<rdfs:seeAlso rdf:resource="&java-se-6;JavaxXmlTransform"/>
		<rdfs:seeAlso rdf:resource="&java-se-6;JavaxXmlBind"/>
		<rdfs:seeAlso rdf:resource="&java-se-6;JavaLang"/>
		<rdfs:seeAlso rdf:resource="&java-se-6;JavaUtilConcurrent"/>
		<rdfs:seeAlso rdf:resource="&java-se-6;JavaSecurity"/>
		<rdfs:seeAlso rdf:resource="&java-se-6;JavaxXmlNamespace"/>
		<rdfs:seeAlso rdf:resource="&java-se-6;JavaNet"/>
		<rdfs:seeAlso rdf:resource="&java-se-6;JavaxXmlWsHandler"/>
		<rdfs:seeAlso rdf:resource="&java-se-6;JavaLangAnnotation"/>
		<rdfs:seeAlso rdf:resource="&java-se-6;JavaUtil"/>
		<rdfs:comment xml:lang="en">Java API part implementing the javax.xml.ws package for Java SE 6</rdfs:comment>
	</owl:Class>
	<owl:Class rdf:about="&java-se-6;JavaxXmlWsHandler">
		<rdfs:subClassOf rdf:resource="&java;JavaAPIPart"/>
		<rdfs:seeAlso rdf:resource="&java-se-6;JavaLang"/>
		<rdfs:seeAlso rdf:resource="&java-se-6;JavaxXmlWs"/>
		<rdfs:seeAlso rdf:resource="&java-se-6;JavaUtil"/>
		<rdfs:seeAlso rdf:resource="&java-se-6;JavaxXmlNamespace"/>
		<rdfs:comment xml:lang="en">Java API part implementing the javax.xml.ws.handler package for Java SE 6</rdfs:comment>
	</owl:Class>
	<owl:Class rdf:about="&java-se-6;JavaxXmlWsHandlerSoap">
		<rdfs:subClassOf rdf:resource="&java;JavaAPIPart"/>
		<rdfs:seeAlso rdf:resource="&java-se-6;JavaxXmlBind"/>
		<rdfs:seeAlso rdf:resource="&java-se-6;JavaxXmlWsHandler"/>
		<rdfs:seeAlso rdf:resource="&java-se-6;JavaUtil"/>
		<rdfs:seeAlso rdf:resource="&java-se-6;JavaxXmlSoap"/>
		<rdfs:seeAlso rdf:resource="&java-se-6;JavaxXmlNamespace"/>
		<rdfs:comment xml:lang="en">Java API part implementing the javax.xml.ws.handler.soap package for Java SE 6</rdfs:comment>
	</owl:Class>
	<owl:Class rdf:about="&java-se-6;JavaxXmlWsHttp">
		<rdfs:subClassOf rdf:resource="&java;JavaAPIPart"/>
		<rdfs:seeAlso rdf:resource="&java-se-6;JavaLang"/>
		<rdfs:seeAlso rdf:resource="&java-se-6;JavaxXmlWs"/>
		<rdfs:comment xml:lang="en">Java API part implementing the javax.xml.ws.http package for Java SE 6</rdfs:comment>
	</owl:Class>
	<owl:Class rdf:about="&java-se-6;JavaxXmlWsSoap">
		<rdfs:subClassOf rdf:resource="&java;JavaAPIPart"/>
		<rdfs:seeAlso rdf:resource="&java-se-6;JavaLang"/>
		<rdfs:seeAlso rdf:resource="&java-se-6;JavaxXmlWs"/>
		<rdfs:seeAlso rdf:resource="&java-se-6;JavaLangAnnotation"/>
		<rdfs:seeAlso rdf:resource="&java-se-6;JavaUtil"/>
		<rdfs:seeAlso rdf:resource="&java-se-6;JavaxXmlSoap"/>
		<rdfs:comment xml:lang="en">Java API part implementing the javax.xml.ws.soap package for Java SE 6</rdfs:comment>
	</owl:Class>
	<owl:Class rdf:about="&java-se-6;JavaxXmlWsSpi">
		<rdfs:subClassOf rdf:resource="&java;JavaAPIPart"/>
		<rdfs:seeAlso rdf:resource="&java-se-6;JavaxXmlTransform"/>
		<rdfs:seeAlso rdf:resource="&java-se-6;JavaxXmlWsWsaddressing"/>
		<rdfs:seeAlso rdf:resource="&java-se-6;JavaxXmlBind"/>
		<rdfs:seeAlso rdf:resource="&java-se-6;JavaUtilConcurrent"/>
		<rdfs:seeAlso rdf:resource="&java-se-6;JavaLang"/>
		<rdfs:seeAlso rdf:resource="&java-se-6;JavaxXmlNamespace"/>
		<rdfs:seeAlso rdf:resource="&java-se-6;JavaNet"/>
		<rdfs:seeAlso rdf:resource="&java-se-6;JavaxXmlWsHandler"/>
		<rdfs:seeAlso rdf:resource="&java-se-6;JavaxXmlWs"/>
		<rdfs:seeAlso rdf:resource="&java-se-6;JavaLangAnnotation"/>
		<rdfs:seeAlso rdf:resource="&java-se-6;JavaUtil"/>
		<rdfs:comment xml:lang="en">Java API part implementing the javax.xml.ws.spi package for Java SE 6</rdfs:comment>
	</owl:Class>
	<owl:Class rdf:about="&java-se-6;JavaxXmlWsWsaddressing">
		<rdfs:subClassOf rdf:resource="&java;JavaAPIPart"/>
		<rdfs:seeAlso rdf:resource="&java-se-6;JavaxXmlTransform"/>
		<rdfs:seeAlso rdf:resource="&java-se-6;OrgW3cDom"/>
		<rdfs:seeAlso rdf:resource="&java-se-6;JavaLang"/>
		<rdfs:seeAlso rdf:resource="&java-se-6;JavaxXmlWs"/>
		<rdfs:seeAlso rdf:resource="&java-se-6;JavaxXmlNamespace"/>
		<rdfs:comment xml:lang="en">Java API part implementing the javax.xml.ws.wsaddressing package for Java SE 6</rdfs:comment>
	</owl:Class>
	<owl:Class rdf:about="&java-se-6;JavaxXmlXpath">
		<rdfs:subClassOf rdf:resource="&j2se-5_0;JavaxXmlXpath"/>
		<rdfs:seeAlso rdf:resource="&java-se-6;JavaLang"/>
		<rdfs:seeAlso rdf:resource="&java-se-6;OrgXmlSax"/>
		<rdfs:seeAlso rdf:resource="&java-se-6;JavaUtil"/>
		<rdfs:seeAlso rdf:resource="&java-se-6;JavaIo"/>
		<rdfs:seeAlso rdf:resource="&java-se-6;JavaxXmlNamespace"/>
		<rdfs:comment xml:lang="en">Java API part implementing the javax.xml.xpath package for Java SE 6</rdfs:comment>
	</owl:Class>
	<owl:Class rdf:about="&java-se-6;JavaxActivation">
		<rdfs:subClassOf rdf:resource="&java;JavaAPIPart"/>
		<rdfs:seeAlso rdf:resource="&java-se-6;JavaAwtDatatransfer"/>
		<rdfs:seeAlso rdf:resource="&java-se-6;JavaLang"/>
		<rdfs:seeAlso rdf:resource="&java-se-6;JavaIo"/>
		<rdfs:seeAlso rdf:resource="&java-se-6;JavaNet"/>
		<rdfs:seeAlso rdf:resource="&java-se-6;JavaUtil"/>
		<rdfs:comment xml:lang="en">Java API part implementing the javax.activation package for Java SE 6</rdfs:comment>
	</owl:Class>
	<owl:Class rdf:about="&java-se-6;JavaxActivity">
		<owl:equivalentClass rdf:resource="&j2se-5_0;JavaxActivity"/>
		<rdfs:subClassOf rdf:resource="&java;JavaAPIPart"/>
		<rdfs:seeAlso rdf:resource="&java-se-6;JavaLang"/>
		<rdfs:seeAlso rdf:resource="&java-se-6;JavaRmi"/>
		<rdfs:comment xml:lang="en">Java API part implementing the javax.activity package for Java SE 6</rdfs:comment>
	</owl:Class>
	<owl:Class rdf:about="&java-se-6;JavaxAnnotation">
		<rdfs:subClassOf rdf:resource="&java;JavaAPIPart"/>
		<rdfs:seeAlso rdf:resource="&java-se-6;JavaLang"/>
		<rdfs:seeAlso rdf:resource="&java-se-6;JavaLangAnnotation"/>
		<rdfs:comment xml:lang="en">Java API part implementing the javax.annotation package for Java SE 6</rdfs:comment>
	</owl:Class>
	<owl:Class rdf:about="&java-se-6;JavaxAnnotationProcessing">
		<rdfs:subClassOf rdf:resource="&java;JavaAPIPart"/>
		<rdfs:seeAlso rdf:resource="&java-se-6;JavaxLangModelUtil"/>
		<rdfs:seeAlso rdf:resource="&java-se-6;JavaLang"/>
		<rdfs:seeAlso rdf:resource="&java-se-6;JavaIo"/>
		<rdfs:seeAlso rdf:resource="&java-se-6;JavaxLangModel"/>
		<rdfs:seeAlso rdf:resource="&java-se-6;JavaxTools"/>
		<rdfs:seeAlso rdf:resource="&java-se-6;JavaLangAnnotation"/>
		<rdfs:seeAlso rdf:resource="&java-se-6;JavaxLangModelElement"/>
		<rdfs:seeAlso rdf:resource="&java-se-6;JavaUtil"/>
		<rdfs:comment xml:lang="en">Java API part implementing the javax.annotation.processing package for Java SE 6</rdfs:comment>
	</owl:Class>
	<owl:Class rdf:about="&java-se-6;JavaxLangModel">
		<rdfs:subClassOf rdf:resource="&java;JavaAPIPart"/>
		<rdfs:seeAlso rdf:resource="&java-se-6;JavaLang"/>
		<rdfs:comment xml:lang="en">Java API part implementing the javax.lang.model package for Java SE 6</rdfs:comment>
	</owl:Class>
	<owl:Class rdf:about="&java-se-6;JavaxLangModelElement">
		<rdfs:subClassOf rdf:resource="&java;JavaAPIPart"/>
		<rdfs:seeAlso rdf:resource="&java-se-6;JavaLang"/>
		<rdfs:seeAlso rdf:resource="&java-se-6;JavaxLangModelType"/>
		<rdfs:seeAlso rdf:resource="&java-se-6;JavaLangAnnotation"/>
		<rdfs:seeAlso rdf:resource="&java-se-6;JavaUtil"/>
		<rdfs:comment xml:lang="en">Java API part implementing the javax.lang.model.element package for Java SE 6</rdfs:comment>
	</owl:Class>
	<owl:Class rdf:about="&java-se-6;JavaxLangModelUtil">
		<rdfs:subClassOf rdf:resource="&java;JavaAPIPart"/>
		<rdfs:seeAlso rdf:resource="&java-se-6;JavaLang"/>
		<rdfs:seeAlso rdf:resource="&java-se-6;JavaIo"/>
		<rdfs:seeAlso rdf:resource="&java-se-6;JavaxLangModelType"/>
		<rdfs:seeAlso rdf:resource="&java-se-6;JavaUtil"/>
		<rdfs:seeAlso rdf:resource="&java-se-6;JavaxLangModelElement"/>
		<rdfs:comment xml:lang="en">Java API part implementing the javax.lang.model.util package for Java SE 6</rdfs:comment>
	</owl:Class>
	<owl:Class rdf:about="&java-se-6;JavaxLangModelType">
		<rdfs:subClassOf rdf:resource="&java;JavaAPIPart"/>
		<rdfs:seeAlso rdf:resource="&java-se-6;JavaLang"/>
		<rdfs:seeAlso rdf:resource="&java-se-6;JavaxLangModelElement"/>
		<rdfs:seeAlso rdf:resource="&java-se-6;JavaUtil"/>
		<rdfs:comment xml:lang="en">Java API part implementing the javax.lang.model.type package for Java SE 6</rdfs:comment>
	</owl:Class>
	<owl:Class rdf:about="&java-se-6;JavaxTools">
		<rdfs:subClassOf rdf:resource="&java;JavaAPIPart"/>
		<rdfs:seeAlso rdf:resource="&java-se-6;JavaLang"/>
		<rdfs:seeAlso rdf:resource="&java-se-6;JavaUtilConcurrent"/>
		<rdfs:seeAlso rdf:resource="&java-se-6;JavaNioCharset"/>
		<rdfs:seeAlso rdf:resource="&java-se-6;JavaIo"/>
		<rdfs:seeAlso rdf:resource="&java-se-6;JavaNet"/>
		<rdfs:seeAlso rdf:resource="&java-se-6;JavaxLangModelElement"/>
		<rdfs:seeAlso rdf:resource="&java-se-6;JavaUtil"/>
		<rdfs:comment xml:lang="en">Java API part implementing the javax.tools package for Java SE 6</rdfs:comment>
	</owl:Class>
	<owl:Class rdf:about="&java-se-6;JavaxImageio">
		<rdfs:subClassOf rdf:resource="&j2se-5_0;JavaxImageio"/>
		<rdfs:seeAlso rdf:resource="&java-se-6;JavaLang"/>
		<rdfs:seeAlso rdf:resource="&java-se-6;JavaIo"/>
		<rdfs:seeAlso rdf:resource="&java-se-6;JavaAwtImage"/>
		<rdfs:seeAlso rdf:resource="&java-se-6;JavaAwtColor"/>
		<rdfs:seeAlso rdf:resource="&java-se-6;JavaxImageioSpi"/>
		<rdfs:seeAlso rdf:resource="&java-se-6;JavaUtil"/>
		<rdfs:seeAlso rdf:resource="&java-se-6;JavaxImageioMetadata"/>
		<rdfs:seeAlso rdf:resource="&java-se-6;JavaxImageioEvent"/>
		<rdfs:seeAlso rdf:resource="&java-se-6;JavaAwt"/>
		<rdfs:seeAlso rdf:resource="&java-se-6;JavaxImageioStream"/>
		<rdfs:seeAlso rdf:resource="&java-se-6;JavaNet"/>
		<rdfs:comment xml:lang="en">Java API part implementing the javax.imageio package for Java SE 6</rdfs:comment>
	</owl:Class>
	<owl:Class rdf:about="&java-se-6;JavaxImageioMetadata">
		<owl:equivalentClass rdf:resource="&j2se-5_0;JavaxImageioMetadata"/>
		<rdfs:subClassOf rdf:resource="&java;JavaAPIPart"/>
		<rdfs:seeAlso rdf:resource="&java-se-6;OrgW3cDom"/>
		<rdfs:seeAlso rdf:resource="&java-se-6;JavaLang"/>
		<rdfs:seeAlso rdf:resource="&java-se-6;JavaxImageio"/>
		<rdfs:seeAlso rdf:resource="&java-se-6;JavaUtil"/>
		<rdfs:comment xml:lang="en">Java API part implementing the javax.imageio.metadata package for Java SE 6</rdfs:comment>
	</owl:Class>
	<owl:Class rdf:about="&java-se-6;JavaxImageioStream">
		<owl:equivalentClass rdf:resource="&j2se-5_0;JavaxImageioStream"/>
		<rdfs:subClassOf rdf:resource="&java;JavaAPIPart"/>
		<rdfs:seeAlso rdf:resource="&java-se-6;JavaLang"/>
		<rdfs:seeAlso rdf:resource="&java-se-6;JavaNio"/>
		<rdfs:seeAlso rdf:resource="&java-se-6;JavaIo"/>
		<rdfs:comment xml:lang="en">Java API part implementing the javax.imageio.stream package for Java SE 6</rdfs:comment>
	</owl:Class>
	<owl:Class rdf:about="&java-se-6;JavaxImageioSpi">
		<owl:equivalentClass rdf:resource="&j2se-5_0;JavaxImageioSpi"/>
		<rdfs:subClassOf rdf:resource="&java;JavaAPIPart"/>
		<rdfs:seeAlso rdf:resource="&java-se-6;JavaLang"/>
		<rdfs:seeAlso rdf:resource="&java-se-6;JavaIo"/>
		<rdfs:seeAlso rdf:resource="&java-se-6;JavaxImageioStream"/>
		<rdfs:seeAlso rdf:resource="&java-se-6;JavaAwtImage"/>
		<rdfs:seeAlso rdf:resource="&java-se-6;JavaxImageio"/>
		<rdfs:seeAlso rdf:resource="&java-se-6;JavaUtil"/>
		<rdfs:seeAlso rdf:resource="&java-se-6;JavaxImageioMetadata"/>
		<rdfs:comment xml:lang="en">Java API part implementing the javax.imageio.spi package for Java SE 6</rdfs:comment>
	</owl:Class>
	<owl:Class rdf:about="&java-se-6;JavaxImageioEvent">
		<owl:equivalentClass rdf:resource="&j2se-5_0;JavaxImageioEvent"/>
		<rdfs:subClassOf rdf:resource="&java;JavaAPIPart"/>
		<rdfs:seeAlso rdf:resource="&java-se-6;JavaAwtImage"/>
		<rdfs:seeAlso rdf:resource="&java-se-6;JavaLang"/>
		<rdfs:seeAlso rdf:resource="&java-se-6;JavaxImageio"/>
		<rdfs:seeAlso rdf:resource="&java-se-6;JavaUtil"/>
		<rdfs:comment xml:lang="en">Java API part implementing the javax.imageio.event package for Java SE 6</rdfs:comment>
	</owl:Class>
	<owl:Class rdf:about="&java-se-6;JavaxImageioPluginsBmp">
		<owl:equivalentClass rdf:resource="&j2se-5_0;JavaxImageioPluginsBmp"/>
		<rdfs:subClassOf rdf:resource="&java;JavaAPIPart"/>
		<rdfs:seeAlso rdf:resource="&java-se-6;JavaxImageio"/>
		<rdfs:seeAlso rdf:resource="&java-se-6;JavaUtil"/>
		<rdfs:comment xml:lang="en">Java API part implementing the javax.imageio.plugins.bmp package for Java SE 6</rdfs:comment>
	</owl:Class>
	<owl:Class rdf:about="&java-se-6;JavaxImageioPluginsJpeg">
		<owl:equivalentClass rdf:resource="&j2se-5_0;JavaxImageioPluginsJpeg"/>
		<rdfs:subClassOf rdf:resource="&java;JavaAPIPart"/>
		<rdfs:seeAlso rdf:resource="&java-se-6;JavaLang"/>
		<rdfs:seeAlso rdf:resource="&java-se-6;JavaxImageio"/>
		<rdfs:seeAlso rdf:resource="&java-se-6;JavaUtil"/>
		<rdfs:comment xml:lang="en">Java API part implementing the javax.imageio.plugins.jpeg package for Java SE 6</rdfs:comment>
	</owl:Class>
	<owl:Class rdf:about="&java-se-6;JavaxJws">
		<rdfs:subClassOf rdf:resource="&java;JavaAPIPart"/>
		<rdfs:seeAlso rdf:resource="&java-se-6;JavaLang"/>
		<rdfs:seeAlso rdf:resource="&java-se-6;JavaLangAnnotation"/>
		<rdfs:comment xml:lang="en">Java API part implementing the javax.jws package for Java SE 6</rdfs:comment>
	</owl:Class>
	<owl:Class rdf:about="&java-se-6;JavaxJwsSoap">
		<rdfs:subClassOf rdf:resource="&java;JavaAPIPart"/>
		<rdfs:seeAlso rdf:resource="&java-se-6;JavaLang"/>
		<rdfs:seeAlso rdf:resource="&java-se-6;JavaLangAnnotation"/>
		<rdfs:comment xml:lang="en">Java API part implementing the javax.jws.soap package for Java SE 6</rdfs:comment>
	</owl:Class>
	<owl:Class rdf:about="&java-se-6;JavaxRmi">
		<owl:equivalentClass rdf:resource="&j2se-5_0;JavaxRmi"/>
		<rdfs:subClassOf rdf:resource="&java;JavaAPIPart"/>
		<rdfs:seeAlso rdf:resource="&java-se-6;JavaLang"/>
		<rdfs:seeAlso rdf:resource="&java-se-6;JavaRmi"/>
		<rdfs:comment xml:lang="en">Java API part implementing the javax.rmi package for Java SE 6</rdfs:comment>
	</owl:Class>
	<owl:Class rdf:about="&java-se-6;JavaxRmiCORBA">
		<owl:equivalentClass rdf:resource="&j2se-5_0;JavaxRmiCORBA"/>
		<rdfs:subClassOf rdf:resource="&java;JavaAPIPart"/>
		<rdfs:seeAlso rdf:resource="&java-se-6;OrgOmgCORBAPortable"/>
		<rdfs:seeAlso rdf:resource="&java-se-6;OrgOmgSendingContext"/>
		<rdfs:seeAlso rdf:resource="&java-se-6;JavaLang"/>
		<rdfs:seeAlso rdf:resource="&java-se-6;JavaIo"/>
		<rdfs:seeAlso rdf:resource="&java-se-6;JavaRmi"/>
		<rdfs:seeAlso rdf:resource="&java-se-6;OrgOmgCORBA_2_3Portable"/>
		<rdfs:seeAlso rdf:resource="&java-se-6;OrgOmgCORBA"/>
		<rdfs:comment xml:lang="en">Java API part implementing the javax.rmi.CORBA package for Java SE 6</rdfs:comment>
	</owl:Class>
	<owl:Class rdf:about="&java-se-6;JavaxRmiSsl">
		<owl:equivalentClass rdf:resource="&j2se-5_0;JavaxRmiSsl"/>
		<rdfs:subClassOf rdf:resource="&java;JavaAPIPart"/>
		<rdfs:seeAlso rdf:resource="&java-se-6;JavaNet"/>
		<rdfs:seeAlso rdf:resource="&java-se-6;JavaLang"/>
		<rdfs:seeAlso rdf:resource="&java-se-6;JavaIo"/>
		<rdfs:seeAlso rdf:resource="&java-se-6;JavaRmiServer"/>
		<rdfs:comment xml:lang="en">Java API part implementing the javax.rmi.ssl package for Java SE 6</rdfs:comment>
	</owl:Class>
	<owl:Class rdf:about="&java-se-6;JavaxNaming">
		<rdfs:subClassOf rdf:resource="&j2se-5_0;JavaxNaming"/>
		<rdfs:seeAlso rdf:resource="&java-se-6;JavaLang"/>
		<rdfs:seeAlso rdf:resource="&java-se-6;JavaIo"/>
		<rdfs:seeAlso rdf:resource="&java-se-6;JavaUtil"/>
		<rdfs:comment xml:lang="en">Java API part implementing the javax.naming package for Java SE 6</rdfs:comment>
	</owl:Class>
	<owl:Class rdf:about="&java-se-6;JavaxNamingDirectory">
		<rdfs:subClassOf rdf:resource="&j2se-5_0;JavaxNamingDirectory"/>
		<rdfs:seeAlso rdf:resource="&java-se-6;JavaLang"/>
		<rdfs:seeAlso rdf:resource="&java-se-6;JavaIo"/>
		<rdfs:seeAlso rdf:resource="&java-se-6;JavaxNaming"/>
		<rdfs:seeAlso rdf:resource="&java-se-6;JavaUtil"/>
		<rdfs:comment xml:lang="en">Java API part implementing the javax.naming.directory package for Java SE 6</rdfs:comment>
	</owl:Class>
	<owl:Class rdf:about="&java-se-6;JavaxNamingEvent">
		<owl:equivalentClass rdf:resource="&j2se-5_0;JavaxNamingEvent"/>
		<rdfs:subClassOf rdf:resource="&java;JavaAPIPart"/>
		<rdfs:seeAlso rdf:resource="&java-se-6;JavaLang"/>
		<rdfs:seeAlso rdf:resource="&java-se-6;JavaxNamingDirectory"/>
		<rdfs:seeAlso rdf:resource="&java-se-6;JavaxNaming"/>
		<rdfs:seeAlso rdf:resource="&java-se-6;JavaUtil"/>
		<rdfs:comment xml:lang="en">Java API part implementing the javax.naming.event package for Java SE 6</rdfs:comment>
	</owl:Class>
	<owl:Class rdf:about="&java-se-6;JavaxNamingLdap">
		<rdfs:subClassOf rdf:resource="&j2se-5_0;JavaxNamingLdap"/>
		<rdfs:seeAlso rdf:resource="&java-se-6;JavaxNetSsl"/>
		<rdfs:seeAlso rdf:resource="&java-se-6;JavaLang"/>
		<rdfs:seeAlso rdf:resource="&java-se-6;JavaxNamingEvent"/>
		<rdfs:seeAlso rdf:resource="&java-se-6;JavaIo"/>
		<rdfs:seeAlso rdf:resource="&java-se-6;JavaxNamingDirectory"/>
		<rdfs:seeAlso rdf:resource="&java-se-6;JavaxNaming"/>
		<rdfs:seeAlso rdf:resource="&java-se-6;JavaUtil"/>
		<rdfs:comment xml:lang="en">Java API part implementing the javax.naming.ldap package for Java SE 6</rdfs:comment>
	</owl:Class>
	<owl:Class rdf:about="&java-se-6;JavaxNamingSpi">
		<owl:equivalentClass rdf:resource="&j2se-5_0;JavaxNamingSpi"/>
		<rdfs:subClassOf rdf:resource="&java;JavaAPIPart"/>
		<rdfs:seeAlso rdf:resource="&java-se-6;JavaLang"/>
		<rdfs:seeAlso rdf:resource="&java-se-6;JavaxNamingDirectory"/>
		<rdfs:seeAlso rdf:resource="&java-se-6;JavaxNaming"/>
		<rdfs:seeAlso rdf:resource="&java-se-6;JavaIo"/>
		<rdfs:seeAlso rdf:resource="&java-se-6;JavaUtil"/>
		<rdfs:comment xml:lang="en">Java API part implementing the javax.naming.spi package for Java SE 6</rdfs:comment>
	</owl:Class>
	<owl:Class rdf:about="&java-se-6;JavaxPrint">
		<owl:equivalentClass rdf:resource="&j2se-5_0;JavaxPrint"/>
		<rdfs:subClassOf rdf:resource="&java;JavaAPIPart"/>
		<rdfs:seeAlso rdf:resource="&java-se-6;JavaAwt"/>
		<rdfs:seeAlso rdf:resource="&java-se-6;JavaxPrintAttribute"/>
		<rdfs:seeAlso rdf:resource="&java-se-6;JavaLang"/>
		<rdfs:seeAlso rdf:resource="&java-se-6;JavaIo"/>
		<rdfs:seeAlso rdf:resource="&java-se-6;JavaNet"/>
		<rdfs:seeAlso rdf:resource="&java-se-6;JavaxPrintEvent"/>
		<rdfs:comment xml:lang="en">Java API part implementing the javax.print package for Java SE 6</rdfs:comment>
	</owl:Class>
	<owl:Class rdf:about="&java-se-6;JavaxPrintAttribute">
		<owl:equivalentClass rdf:resource="&j2se-5_0;JavaxPrintAttribute"/>
		<rdfs:subClassOf rdf:resource="&java;JavaAPIPart"/>
		<rdfs:seeAlso rdf:resource="&java-se-6;JavaNet"/>
		<rdfs:seeAlso rdf:resource="&java-se-6;JavaLang"/>
		<rdfs:seeAlso rdf:resource="&java-se-6;JavaIo"/>
		<rdfs:seeAlso rdf:resource="&java-se-6;JavaUtil"/>
		<rdfs:comment xml:lang="en">Java API part implementing the javax.print.attribute package for Java SE 6</rdfs:comment>
	</owl:Class>
	<owl:Class rdf:about="&java-se-6;JavaxPrintAttributeStandard">
		<owl:equivalentClass rdf:resource="&j2se-5_0;JavaxPrintAttributeStandard"/>
		<rdfs:subClassOf rdf:resource="&java;JavaAPIPart"/>
		<rdfs:seeAlso rdf:resource="&java-se-6;JavaxPrintAttribute"/>
		<rdfs:seeAlso rdf:resource="&java-se-6;JavaLang"/>
		<rdfs:seeAlso rdf:resource="&java-se-6;JavaUtil"/>
		<rdfs:seeAlso rdf:resource="&java-se-6;JavaNet"/>
		<rdfs:comment xml:lang="en">Java API part implementing the javax.print.attribute.standard package for Java SE 6</rdfs:comment>
	</owl:Class>
	<owl:Class rdf:about="&java-se-6;JavaxPrintEvent">
		<owl:equivalentClass rdf:resource="&j2se-5_0;JavaxPrintEvent"/>
		<rdfs:subClassOf rdf:resource="&java;JavaAPIPart"/>
		<rdfs:seeAlso rdf:resource="&java-se-6;JavaLang"/>
		<rdfs:seeAlso rdf:resource="&java-se-6;JavaxPrintAttribute"/>
		<rdfs:seeAlso rdf:resource="&java-se-6;JavaxPrint"/>
		<rdfs:seeAlso rdf:resource="&java-se-6;JavaUtil"/>
		<rdfs:comment xml:lang="en">Java API part implementing the javax.print.event package for Java SE 6</rdfs:comment>
	</owl:Class>
	<owl:Class rdf:about="&java-se-6;JavaxScript">
		<rdfs:subClassOf rdf:resource="&java;JavaAPIPart"/>
		<rdfs:seeAlso rdf:resource="&java-se-6;JavaLang"/>
		<rdfs:seeAlso rdf:resource="&java-se-6;JavaIo"/>
		<rdfs:seeAlso rdf:resource="&java-se-6;JavaUtil"/>
		<rdfs:comment xml:lang="en">Java API part implementing the javax.script package for Java SE 6</rdfs:comment>
	</owl:Class>
	<owl:Class rdf:about="&java-se-6;JavaxSmartcardio">
		<rdfs:subClassOf rdf:resource="&java;JavaAPIPart"/>
		<rdfs:seeAlso rdf:resource="&java-se-6;JavaLang"/>
		<rdfs:seeAlso rdf:resource="&java-se-6;JavaNio"/>
		<rdfs:seeAlso rdf:resource="&java-se-6;JavaSecurity"/>
		<rdfs:seeAlso rdf:resource="&java-se-6;JavaUtil"/>
		<rdfs:seeAlso rdf:resource="&java-se-6;JavaIo"/>
		<rdfs:comment xml:lang="en">Java API part implementing the javax.smartcardio package for Java SE 6</rdfs:comment>
	</owl:Class>
	<owl:Class rdf:about="&java-se-6;JavaxSoundMidi">
		<owl:equivalentClass rdf:resource="&j2se-5_0;JavaxSoundMidi"/>
		<rdfs:subClassOf rdf:resource="&java;JavaAPIPart"/>
		<rdfs:seeAlso rdf:resource="&java-se-6;JavaLang"/>
		<rdfs:seeAlso rdf:resource="&java-se-6;JavaIo"/>
		<rdfs:seeAlso rdf:resource="&java-se-6;JavaNet"/>
		<rdfs:seeAlso rdf:resource="&java-se-6;JavaUtil"/>
		<rdfs:comment xml:lang="en">Java API part implementing the javax.sound.midi package for Java SE 6</rdfs:comment>
	</owl:Class>
	<owl:Class rdf:about="&java-se-6;JavaxSoundMidiSpi">
		<owl:equivalentClass rdf:resource="&j2se-5_0;JavaxSoundMidiSpi"/>
		<rdfs:subClassOf rdf:resource="&java;JavaAPIPart"/>
		<rdfs:seeAlso rdf:resource="&java-se-6;JavaNet"/>
		<rdfs:seeAlso rdf:resource="&java-se-6;JavaLang"/>
		<rdfs:seeAlso rdf:resource="&java-se-6;JavaxSoundMidi"/>
		<rdfs:seeAlso rdf:resource="&java-se-6;JavaIo"/>
		<rdfs:comment xml:lang="en">Java API part implementing the javax.sound.midi.spi package for Java SE 6</rdfs:comment>
	</owl:Class>
	<owl:Class rdf:about="&java-se-6;JavaxSoundSampled">
		<owl:equivalentClass rdf:resource="&j2se-5_0;JavaxSoundSampled"/>
		<rdfs:subClassOf rdf:resource="&java;JavaAPIPart"/>
		<rdfs:seeAlso rdf:resource="&java-se-6;JavaLang"/>
		<rdfs:seeAlso rdf:resource="&java-se-6;JavaSecurity"/>
		<rdfs:seeAlso rdf:resource="&java-se-6;JavaIo"/>
		<rdfs:seeAlso rdf:resource="&java-se-6;JavaNet"/>
		<rdfs:seeAlso rdf:resource="&java-se-6;JavaUtil"/>
		<rdfs:comment xml:lang="en">Java API part implementing the javax.sound.sampled package for Java SE 6</rdfs:comment>
	</owl:Class>
	<owl:Class rdf:about="&java-se-6;JavaxSoundSampledSpi">
		<owl:equivalentClass rdf:resource="&j2se-5_0;JavaxSoundSampledSpi"/>
		<rdfs:subClassOf rdf:resource="&java;JavaAPIPart"/>
		<rdfs:seeAlso rdf:resource="&java-se-6;JavaxSoundSampled"/>
		<rdfs:seeAlso rdf:resource="&java-se-6;JavaLang"/>
		<rdfs:seeAlso rdf:resource="&java-se-6;JavaIo"/>
		<rdfs:seeAlso rdf:resource="&java-se-6;JavaNet"/>
		<rdfs:comment xml:lang="en">Java API part implementing the javax.sound.sampled.spi package for Java SE 6</rdfs:comment>
	</owl:Class>
	<owl:Class rdf:about="&java-se-6;JavaxSql">
		<rdfs:subClassOf rdf:resource="&j2se-5_0;JavaxSql"/>
		<rdfs:seeAlso rdf:resource="&java-se-6;JavaLang"/>
		<rdfs:seeAlso rdf:resource="&java-se-6;JavaxTransactionXa"/>
		<rdfs:seeAlso rdf:resource="&java-se-6;JavaIo"/>
		<rdfs:seeAlso rdf:resource="&java-se-6;JavaUtil"/>
		<rdfs:seeAlso rdf:resource="&java-se-6;JavaNet"/>
		<rdfs:seeAlso rdf:resource="&java-se-6;JavaSql"/>
		<rdfs:seeAlso rdf:resource="&java-se-6;JavaMath"/>
		<rdfs:comment xml:lang="en">Java API part implementing the javax.sql package for Java SE 6</rdfs:comment>
	</owl:Class>
	<owl:Class rdf:about="&java-se-6;JavaxSqlRowset">
		<rdfs:subClassOf rdf:resource="&j2se-5_0;JavaxSqlRowset"/>
		<rdfs:seeAlso rdf:resource="&java-se-6;JavaLang"/>
		<rdfs:seeAlso rdf:resource="&java-se-6;JavaxSql"/>
		<rdfs:seeAlso rdf:resource="&java-se-6;JavaxSqlRowsetSpi"/>
		<rdfs:seeAlso rdf:resource="&java-se-6;JavaIo"/>
		<rdfs:seeAlso rdf:resource="&java-se-6;JavaUtil"/>
		<rdfs:seeAlso rdf:resource="&java-se-6;JavaNet"/>
		<rdfs:seeAlso rdf:resource="&java-se-6;JavaSql"/>
		<rdfs:seeAlso rdf:resource="&java-se-6;JavaMath"/>
		<rdfs:comment xml:lang="en">Java API part implementing the javax.sql.rowset package for Java SE 6</rdfs:comment>
	</owl:Class>
	<owl:Class rdf:about="&java-se-6;JavaxSqlRowsetSpi">
		<rdfs:subClassOf rdf:resource="&j2se-5_0;JavaxSqlRowsetSpi"/>
		<rdfs:seeAlso rdf:resource="&java-se-6;JavaLang"/>
		<rdfs:seeAlso rdf:resource="&java-se-6;JavaxSql"/>
		<rdfs:seeAlso rdf:resource="&java-se-6;JavaUtilLogging"/>
		<rdfs:seeAlso rdf:resource="&java-se-6;JavaIo"/>
		<rdfs:seeAlso rdf:resource="&java-se-6;JavaxSqlRowset"/>
		<rdfs:seeAlso rdf:resource="&java-se-6;JavaSql"/>
		<rdfs:seeAlso rdf:resource="&java-se-6;JavaxNaming"/>
		<rdfs:seeAlso rdf:resource="&java-se-6;JavaUtil"/>
		<rdfs:comment xml:lang="en">Java API part implementing the javax.sql.rowset.spi package for Java SE 6</rdfs:comment>
	</owl:Class>
	<owl:Class rdf:about="&java-se-6;JavaxSqlRowsetSerial">
		<rdfs:subClassOf rdf:resource="&j2se-5_0;JavaxSqlRowsetSerial"/>
		<rdfs:seeAlso rdf:resource="&java-se-6;JavaLang"/>
		<rdfs:seeAlso rdf:resource="&java-se-6;JavaIo"/>
		<rdfs:seeAlso rdf:resource="&java-se-6;JavaUtil"/>
		<rdfs:seeAlso rdf:resource="&java-se-6;JavaNet"/>
		<rdfs:seeAlso rdf:resource="&java-se-6;JavaSql"/>
		<rdfs:seeAlso rdf:resource="&java-se-6;JavaMath"/>
		<rdfs:comment xml:lang="en">Java API part implementing the javax.sql.rowset.serial package for Java SE 6</rdfs:comment>
	</owl:Class>
	<owl:Class rdf:about="&java-se-6;JavaxTransaction">
		<owl:equivalentClass rdf:resource="&j2se-5_0;JavaxTransaction"/>
		<rdfs:subClassOf rdf:resource="&java;JavaAPIPart"/>
		<rdfs:seeAlso rdf:resource="&java-se-6;JavaLang"/>
		<rdfs:seeAlso rdf:resource="&java-se-6;JavaRmi"/>
		<rdfs:comment xml:lang="en">Java API part implementing the javax.transaction package for Java SE 6</rdfs:comment>
	</owl:Class>
	<owl:Class rdf:about="&java-se-6;JavaxTransactionXa">
		<owl:equivalentClass rdf:resource="&j2se-5_0;JavaxTransactionXa"/>
		<rdfs:subClassOf rdf:resource="&java;JavaAPIPart"/>
		<rdfs:seeAlso rdf:resource="&java-se-6;JavaLang"/>
		<rdfs:comment xml:lang="en">Java API part implementing the javax.transaction.xa package for Java SE 6</rdfs:comment>
	</owl:Class>
	<owl:Class rdf:about="&java-se-6;JavaLang">
		<rdfs:subClassOf rdf:resource="&j2se-5_0;JavaLang"/>
		<rdfs:seeAlso rdf:resource="&java-se-6;JavaNio"/>
		<rdfs:seeAlso rdf:resource="&java-se-6;JavaIo"/>
		<rdfs:seeAlso rdf:resource="&java-se-6;JavaUtil"/>
		<rdfs:seeAlso rdf:resource="&java-se-6;JavaNioChannels"/>
		<rdfs:seeAlso rdf:resource="&java-se-6;JavaNioCharset"/>
		<rdfs:seeAlso rdf:resource="&java-se-6;JavaSecurity"/>
		<rdfs:seeAlso rdf:resource="&java-se-6;JavaNet"/>
		<rdfs:seeAlso rdf:resource="&java-se-6;JavaLangReflect"/>
		<rdfs:seeAlso rdf:resource="&java-se-6;JavaLangAnnotation"/>
		<rdfs:comment xml:lang="en">Java API part implementing the java.lang package for Java SE 6</rdfs:comment>
	</owl:Class>
	<owl:Class rdf:about="&java-se-6;JavaLangAnnotation">
		<rdfs:subClassOf rdf:resource="&j2se-5_0;JavaLangAnnotation"/>
		<rdfs:seeAlso rdf:resource="&java-se-6;JavaLang"/>
		<rdfs:seeAlso rdf:resource="&java-se-6;JavaLangReflect"/>
		<rdfs:comment xml:lang="en">Java API part implementing the java.lang.annotation package for Java SE 6</rdfs:comment>
	</owl:Class>
	<owl:Class rdf:about="&java-se-6;JavaLangReflect">
		<owl:equivalentClass rdf:resource="&j2se-5_0;JavaLangReflect"/>
		<rdfs:subClassOf rdf:resource="&java;JavaAPIPart"/>
		<rdfs:seeAlso rdf:resource="&java-se-6;JavaLang"/>
		<rdfs:seeAlso rdf:resource="&java-se-6;JavaSecurity"/>
		<rdfs:seeAlso rdf:resource="&java-se-6;JavaLangAnnotation"/>
		<rdfs:seeAlso rdf:resource="&java-se-6;JavaIo"/>
		<rdfs:comment xml:lang="en">Java API part implementing the java.lang.reflect package for Java SE 6</rdfs:comment>
	</owl:Class>
	<owl:Class rdf:about="&java-se-6;JavaLangInstrument">
		<rdfs:subClassOf rdf:resource="&j2se-5_0;JavaLangInstrument"/>
		<rdfs:seeAlso rdf:resource="&java-se-6;JavaUtilJar"/>
		<rdfs:seeAlso rdf:resource="&java-se-6;JavaLang"/>
		<rdfs:seeAlso rdf:resource="&java-se-6;JavaSecurity"/>
		<rdfs:comment xml:lang="en">Java API part implementing the java.lang.instrument package for Java SE 6</rdfs:comment>
	</owl:Class>
	<owl:Class rdf:about="&java-se-6;JavaLangManagement">
		<rdfs:subClassOf rdf:resource="&j2se-5_0;JavaLangManagement"/>
		<rdfs:seeAlso rdf:resource="&java-se-6;JavaLang"/>
		<rdfs:seeAlso rdf:resource="&java-se-6;JavaxManagement"/>
		<rdfs:seeAlso rdf:resource="&java-se-6;JavaSecurity"/>
		<rdfs:seeAlso rdf:resource="&java-se-6;JavaxManagementOpenmbean"/>
		<rdfs:seeAlso rdf:resource="&java-se-6;JavaUtil"/>
		<rdfs:comment xml:lang="en">Java API part implementing the java.lang.management package for Java SE 6</rdfs:comment>
	</owl:Class>
	<owl:Class rdf:about="&java-se-6;JavaLangRef">
		<owl:equivalentClass rdf:resource="&j2se-5_0;JavaLangRef"/>
		<rdfs:subClassOf rdf:resource="&java;JavaAPIPart"/>
		<rdfs:seeAlso rdf:resource="&java-se-6;JavaLang"/>
		<rdfs:comment xml:lang="en">Java API part implementing the java.lang.ref package for Java SE 6</rdfs:comment>
	</owl:Class>
	<owl:Class rdf:about="&java-se-6;JavaAwt">
		<rdfs:subClassOf rdf:resource="&j2se-5_0;JavaAwt"/>
		<rdfs:seeAlso rdf:resource="&java-se-6;JavaAwtColor"/>
		<rdfs:seeAlso rdf:resource="&java-se-6;JavaAwtDatatransfer"/>
		<rdfs:seeAlso rdf:resource="&java-se-6;JavaLang"/>
		<rdfs:seeAlso rdf:resource="&java-se-6;JavaIo"/>
		<rdfs:seeAlso rdf:resource="&java-se-6;JavaUtil"/>
		<rdfs:seeAlso rdf:resource="&java-se-6;JavaAwtGeom"/>
		<rdfs:seeAlso rdf:resource="&java-se-6;JavaAwtDnd"/>
		<rdfs:seeAlso rdf:resource="&java-se-6;JavaAwtImageRenderable"/>
		<rdfs:seeAlso rdf:resource="&java-se-6;JavaxAccessibility"/>
		<rdfs:seeAlso rdf:resource="&java-se-6;JavaText"/>
		<rdfs:seeAlso rdf:resource="&java-se-6;JavaxSwingText"/>
		<rdfs:seeAlso rdf:resource="&java-se-6;JavaNet"/>
		<rdfs:seeAlso rdf:resource="&java-se-6;JavaAwtIm"/>
		<rdfs:seeAlso rdf:resource="&java-se-6;JavaAwtImage"/>
		<rdfs:seeAlso rdf:resource="&java-se-6;JavaBeans"/>
		<rdfs:seeAlso rdf:resource="&java-se-6;JavaAwtEvent"/>
		<rdfs:seeAlso rdf:resource="&java-se-6;JavaAwtFont"/>
		<rdfs:seeAlso rdf:resource="&java-se-6;JavaSecurity"/>
		<rdfs:comment xml:lang="en">Java API part implementing the java.awt package for Java SE 6</rdfs:comment>
	</owl:Class>
	<owl:Class rdf:about="&java-se-6;JavaAwtPrint">
		<rdfs:subClassOf rdf:resource="&j2se-5_0;JavaAwtPrint"/>
		<rdfs:seeAlso rdf:resource="&java-se-6;JavaAwt"/>
		<rdfs:seeAlso rdf:resource="&java-se-6;JavaxPrintAttribute"/>
		<rdfs:seeAlso rdf:resource="&java-se-6;JavaLang"/>
		<rdfs:seeAlso rdf:resource="&java-se-6;JavaxPrint"/>
		<rdfs:seeAlso rdf:resource="&java-se-6;JavaIo"/>
		<rdfs:comment xml:lang="en">Java API part implementing the java.awt.print package for Java SE 6</rdfs:comment>
	</owl:Class>
	<owl:Class rdf:about="&java-se-6;JavaAwtDatatransfer">
		<owl:equivalentClass rdf:resource="&j2se-5_0;JavaAwtDatatransfer"/>
		<rdfs:subClassOf rdf:resource="&java;JavaAPIPart"/>
		<rdfs:seeAlso rdf:resource="&java-se-6;JavaLang"/>
		<rdfs:seeAlso rdf:resource="&java-se-6;JavaIo"/>
		<rdfs:seeAlso rdf:resource="&java-se-6;JavaUtil"/>
		<rdfs:comment xml:lang="en">Java API part implementing the java.awt.datatransfer package for Java SE 6</rdfs:comment>
	</owl:Class>
	<owl:Class rdf:about="&java-se-6;JavaAwtEvent">
		<rdfs:subClassOf rdf:resource="&j2se-5_0;JavaAwtEvent"/>
		<rdfs:seeAlso rdf:resource="&java-se-6;JavaAwt"/>
		<rdfs:seeAlso rdf:resource="&java-se-6;JavaLang"/>
		<rdfs:seeAlso rdf:resource="&java-se-6;JavaAwtFont"/>
		<rdfs:seeAlso rdf:resource="&java-se-6;JavaText"/>
		<rdfs:seeAlso rdf:resource="&java-se-6;JavaUtil"/>
		<rdfs:comment xml:lang="en">Java API part implementing the java.awt.event package for Java SE 6</rdfs:comment>
	</owl:Class>
	<owl:Class rdf:about="&java-se-6;JavaAwtImage">
		<rdfs:subClassOf rdf:resource="&j2se-5_0;JavaAwtImage"/>
		<rdfs:seeAlso rdf:resource="&java-se-6;JavaAwtGeom"/>
		<rdfs:seeAlso rdf:resource="&java-se-6;JavaAwt"/>
		<rdfs:seeAlso rdf:resource="&java-se-6;JavaLang"/>
		<rdfs:seeAlso rdf:resource="&java-se-6;JavaMath"/>
		<rdfs:seeAlso rdf:resource="&java-se-6;JavaAwtColor"/>
		<rdfs:seeAlso rdf:resource="&java-se-6;JavaUtil"/>
		<rdfs:comment xml:lang="en">Java API part implementing the java.awt.image package for Java SE 6</rdfs:comment>
	</owl:Class>
	<owl:Class rdf:about="&java-se-6;JavaAwtImageRenderable">
		<owl:equivalentClass rdf:resource="&j2se-5_0;JavaAwtImageRenderable"/>
		<rdfs:subClassOf rdf:resource="&java;JavaAPIPart"/>
		<rdfs:seeAlso rdf:resource="&java-se-6;JavaAwtGeom"/>
		<rdfs:seeAlso rdf:resource="&java-se-6;JavaAwt"/>
		<rdfs:seeAlso rdf:resource="&java-se-6;JavaLang"/>
		<rdfs:seeAlso rdf:resource="&java-se-6;JavaIo"/>
		<rdfs:seeAlso rdf:resource="&java-se-6;JavaAwtImage"/>
		<rdfs:seeAlso rdf:resource="&java-se-6;JavaUtil"/>
		<rdfs:comment xml:lang="en">Java API part implementing the java.awt.image.renderable package for Java SE 6</rdfs:comment>
	</owl:Class>
	<owl:Class rdf:about="&java-se-6;JavaAwtGeom">
		<rdfs:subClassOf rdf:resource="&java;JavaAPIPart"/>
		<rdfs:seeAlso rdf:resource="&java-se-6;JavaAwt"/>
		<rdfs:seeAlso rdf:resource="&java-se-6;JavaLang"/>
		<rdfs:seeAlso rdf:resource="&java-se-6;JavaIo"/>
		<rdfs:comment xml:lang="en">Java API part implementing the java.awt.geom package for Java SE 6</rdfs:comment>
	</owl:Class>
	<owl:Class rdf:about="&java-se-6;JavaAwtIm">
		<owl:equivalentClass rdf:resource="&j2se-5_0;JavaAwtIm"/>
		<rdfs:subClassOf rdf:resource="&java;JavaAPIPart"/>
		<rdfs:seeAlso rdf:resource="&java-se-6;JavaText"/>
		<rdfs:seeAlso rdf:resource="&java-se-6;JavaAwt"/>
		<rdfs:seeAlso rdf:resource="&java-se-6;JavaLang"/>
		<rdfs:seeAlso rdf:resource="&java-se-6;JavaAwtFont"/>
		<rdfs:seeAlso rdf:resource="&java-se-6;JavaUtil"/>
		<rdfs:comment xml:lang="en">Java API part implementing the java.awt.im package for Java SE 6</rdfs:comment>
	</owl:Class>
	<owl:Class rdf:about="&java-se-6;JavaAwtImSpi">
		<owl:equivalentClass rdf:resource="&j2se-5_0;JavaAwtImSpi"/>
		<rdfs:subClassOf rdf:resource="&java;JavaAPIPart"/>
		<rdfs:seeAlso rdf:resource="&java-se-6;JavaxSwing"/>
		<rdfs:seeAlso rdf:resource="&java-se-6;JavaText"/>
		<rdfs:seeAlso rdf:resource="&java-se-6;JavaAwt"/>
		<rdfs:seeAlso rdf:resource="&java-se-6;JavaLang"/>
		<rdfs:seeAlso rdf:resource="&java-se-6;JavaAwtFont"/>
		<rdfs:seeAlso rdf:resource="&java-se-6;JavaAwtIm"/>
		<rdfs:seeAlso rdf:resource="&java-se-6;JavaUtil"/>
		<rdfs:comment xml:lang="en">Java API part implementing the java.awt.im.spi package for Java SE 6</rdfs:comment>
	</owl:Class>
	<owl:Class rdf:about="&java-se-6;JavaAwtColor">
		<owl:equivalentClass rdf:resource="&j2se-5_0;JavaAwtColor"/>
		<rdfs:subClassOf rdf:resource="&java;JavaAPIPart"/>
		<rdfs:seeAlso rdf:resource="&java-se-6;JavaLang"/>
		<rdfs:seeAlso rdf:resource="&java-se-6;JavaIo"/>
		<rdfs:comment xml:lang="en">Java API part implementing the java.awt.color package for Java SE 6</rdfs:comment>
	</owl:Class>
	<owl:Class rdf:about="&java-se-6;JavaAwtDnd">
		<owl:equivalentClass rdf:resource="&j2se-5_0;JavaAwtDnd"/>
		<rdfs:subClassOf rdf:resource="&java;JavaAPIPart"/>
		<rdfs:seeAlso rdf:resource="&java-se-6;JavaLang"/>
		<rdfs:seeAlso rdf:resource="&java-se-6;JavaIo"/>
		<rdfs:seeAlso rdf:resource="&java-se-6;JavaUtil"/>
		<rdfs:seeAlso rdf:resource="&java-se-6;JavaAwtEvent"/>
		<rdfs:seeAlso rdf:resource="&java-se-6;JavaAwtDatatransfer"/>
		<rdfs:seeAlso rdf:resource="&java-se-6;JavaAwt"/>
		<rdfs:comment xml:lang="en">Java API part implementing the java.awt.dnd package for Java SE 6</rdfs:comment>
	</owl:Class>
	<owl:Class rdf:about="&java-se-6;JavaAwtFont">
		<rdfs:subClassOf rdf:resource="&j2se-5_0;JavaAwtFont"/>
		<rdfs:seeAlso rdf:resource="&java-se-6;JavaAwtGeom"/>
		<rdfs:seeAlso rdf:resource="&java-se-6;JavaAwt"/>
		<rdfs:seeAlso rdf:resource="&java-se-6;JavaLang"/>
		<rdfs:seeAlso rdf:resource="&java-se-6;JavaIo"/>
		<rdfs:seeAlso rdf:resource="&java-se-6;JavaText"/>
		<rdfs:seeAlso rdf:resource="&java-se-6;JavaUtil"/>
		<rdfs:comment xml:lang="en">Java API part implementing the java.awt.font package for Java SE 6</rdfs:comment>
	</owl:Class>
	<owl:Class rdf:about="&java-se-6;JavaNet">
		<rdfs:subClassOf rdf:resource="&j2se-5_0;JavaNet"/>
		<rdfs:seeAlso rdf:resource="&java-se-6;JavaLang"/>
		<rdfs:seeAlso rdf:resource="&java-se-6;JavaIo"/>
		<rdfs:seeAlso rdf:resource="&java-se-6;JavaUtilJar"/>
		<rdfs:seeAlso rdf:resource="&java-se-6;JavaUtil"/>
		<rdfs:seeAlso rdf:resource="&java-se-6;JavaNioChannels"/>
		<rdfs:seeAlso rdf:resource="&java-se-6;JavaSecurity"/>
		<rdfs:comment xml:lang="en">Java API part implementing the java.net package for Java SE 6</rdfs:comment>
	</owl:Class>
	<owl:Class rdf:about="&java-se-6;JavaIo">
		<rdfs:subClassOf rdf:resource="&j2se-5_0;JavaIo"/>
		<rdfs:seeAlso rdf:resource="&java-se-6;JavaLang"/>
		<rdfs:seeAlso rdf:resource="&java-se-6;JavaNioCharset"/>
		<rdfs:seeAlso rdf:resource="&java-se-6;JavaNio"/>
		<rdfs:seeAlso rdf:resource="&java-se-6;JavaSecurity"/>
		<rdfs:seeAlso rdf:resource="&java-se-6;JavaNet"/>
		<rdfs:seeAlso rdf:resource="&java-se-6;JavaUtil"/>
		<rdfs:seeAlso rdf:resource="&java-se-6;JavaNioChannels"/>
		<rdfs:comment xml:lang="en">Java API part implementing the java.io package for Java SE 6</rdfs:comment>
	</owl:Class>
	<owl:Class rdf:about="&java-se-6;JavaSecurity">
		<rdfs:subClassOf rdf:resource="&j2se-5_0;JavaSecurity"/>
		<rdfs:seeAlso rdf:resource="&java-se-6;JavaSecuritySpec"/>
		<rdfs:seeAlso rdf:resource="&java-se-6;JavaLang"/>
		<rdfs:seeAlso rdf:resource="&java-se-6;JavaNio"/>
		<rdfs:seeAlso rdf:resource="&java-se-6;JavaIo"/>
		<rdfs:seeAlso rdf:resource="&java-se-6;JavaxSecurityAuth"/>
		<rdfs:seeAlso rdf:resource="&java-se-6;JavaUtil"/>
		<rdfs:seeAlso rdf:resource="&java-se-6;JavaxSecurityAuthCallback"/>
		<rdfs:seeAlso rdf:resource="&java-se-6;JavaxSecurityAuthLogin"/>
		<rdfs:seeAlso rdf:resource="&java-se-6;JavaxCrypto"/>
		<rdfs:seeAlso rdf:resource="&java-se-6;JavaNet"/>
		<rdfs:seeAlso rdf:resource="&java-se-6;JavaSecurityCert"/>
		<rdfs:comment xml:lang="en">Java API part implementing the java.security package for Java SE 6</rdfs:comment>
	</owl:Class>
	<owl:Class rdf:about="&java-se-6;JavaSecuritySpec">
		<owl:equivalentClass rdf:resource="&j2se-5_0;JavaSecuritySpec"/>
		<rdfs:subClassOf rdf:resource="&java;JavaAPIPart"/>
		<rdfs:seeAlso rdf:resource="&java-se-6;JavaMath"/>
		<rdfs:seeAlso rdf:resource="&java-se-6;JavaLang"/>
		<rdfs:seeAlso rdf:resource="&java-se-6;JavaSecurity"/>
		<rdfs:seeAlso rdf:resource="&java-se-6;JavaSecurityInterfaces"/>
		<rdfs:comment xml:lang="en">Java API part implementing the java.security.spec package for Java SE 6</rdfs:comment>
	</owl:Class>
	<owl:Class rdf:about="&java-se-6;JavaSecurityCert">
		<owl:equivalentClass rdf:resource="&j2se-5_0;JavaSecurityCert"/>
		<rdfs:subClassOf rdf:resource="&java;JavaAPIPart"/>
		<rdfs:seeAlso rdf:resource="&java-se-6;JavaLang"/>
		<rdfs:seeAlso rdf:resource="&java-se-6;JavaSecurity"/>
		<rdfs:seeAlso rdf:resource="&java-se-6;JavaIo"/>
		<rdfs:seeAlso rdf:resource="&java-se-6;JavaxSecurityAuthX500"/>
		<rdfs:seeAlso rdf:resource="&java-se-6;JavaMath"/>
		<rdfs:seeAlso rdf:resource="&java-se-6;JavaUtil"/>
		<rdfs:comment xml:lang="en">Java API part implementing the java.security.cert package for Java SE 6</rdfs:comment>
	</owl:Class>
	<owl:Class rdf:about="&java-se-6;JavaSecurityAcl">
		<owl:equivalentClass rdf:resource="&j2se-5_0;JavaSecurityAcl"/>
		<rdfs:subClassOf rdf:resource="&java;JavaAPIPart"/>
		<rdfs:seeAlso rdf:resource="&java-se-6;JavaLang"/>
		<rdfs:seeAlso rdf:resource="&java-se-6;JavaSecurity"/>
		<rdfs:seeAlso rdf:resource="&java-se-6;JavaUtil"/>
		<rdfs:comment xml:lang="en">Java API part implementing the java.security.acl package for Java SE 6</rdfs:comment>
	</owl:Class>
	<owl:Class rdf:about="&java-se-6;JavaSecurityInterfaces">
		<owl:equivalentClass rdf:resource="&j2se-5_0;JavaSecurityInterfaces"/>
		<rdfs:subClassOf rdf:resource="&java;JavaAPIPart"/>
		<rdfs:seeAlso rdf:resource="&java-se-6;JavaSecuritySpec"/>
		<rdfs:seeAlso rdf:resource="&java-se-6;JavaMath"/>
		<rdfs:seeAlso rdf:resource="&java-se-6;JavaSecurity"/>
		<rdfs:comment xml:lang="en">Java API part implementing the java.security.interfaces package for Java SE 6</rdfs:comment>
	</owl:Class>
	<owl:Class rdf:about="&java-se-6;JavaMath">
		<rdfs:subClassOf rdf:resource="&j2se-5_0;JavaMath"/>
		<rdfs:seeAlso rdf:resource="&java-se-6;JavaLang"/>
		<rdfs:seeAlso rdf:resource="&java-se-6;JavaUtil"/>
		<rdfs:seeAlso rdf:resource="&java-se-6;JavaIo"/>
		<rdfs:comment xml:lang="en">Java API part implementing the java.math package for Java SE 6</rdfs:comment>
	</owl:Class>
	<owl:Class rdf:about="&java-se-6;JavaNio">
		<rdfs:subClassOf rdf:resource="&j2se-5_0;JavaNio"/>
		<rdfs:seeAlso rdf:resource="&java-se-6;JavaLang"/>
		<rdfs:comment xml:lang="en">Java API part implementing the java.nio package for Java SE 6</rdfs:comment>
	</owl:Class>
	<owl:Class rdf:about="&java-se-6;JavaNioChannels">
		<owl:equivalentClass rdf:resource="&j2se-5_0;JavaNioChannels"/>
		<rdfs:subClassOf rdf:resource="&java;JavaAPIPart"/>
		<rdfs:seeAlso rdf:resource="&java-se-6;JavaLang"/>
		<rdfs:seeAlso rdf:resource="&java-se-6;JavaNioChannelsSpi"/>
		<rdfs:seeAlso rdf:resource="&java-se-6;JavaNioCharset"/>
		<rdfs:seeAlso rdf:resource="&java-se-6;JavaNio"/>
		<rdfs:seeAlso rdf:resource="&java-se-6;JavaIo"/>
		<rdfs:seeAlso rdf:resource="&java-se-6;JavaNet"/>
		<rdfs:seeAlso rdf:resource="&java-se-6;JavaUtil"/>
		<rdfs:comment xml:lang="en">Java API part implementing the java.nio.channels package for Java SE 6</rdfs:comment>
	</owl:Class>
	<owl:Class rdf:about="&java-se-6;JavaNioChannelsSpi">
		<owl:equivalentClass rdf:resource="&j2se-5_0;JavaNioChannelsSpi"/>
		<rdfs:subClassOf rdf:resource="&java;JavaAPIPart"/>
		<rdfs:seeAlso rdf:resource="&java-se-6;JavaLang"/>
		<rdfs:seeAlso rdf:resource="&java-se-6;JavaUtil"/>
		<rdfs:seeAlso rdf:resource="&java-se-6;JavaNioChannels"/>
		<rdfs:comment xml:lang="en">Java API part implementing the java.nio.channels.spi package for Java SE 6</rdfs:comment>
	</owl:Class>
	<owl:Class rdf:about="&java-se-6;JavaNioCharset">
		<owl:equivalentClass rdf:resource="&j2se-5_0;JavaNioCharset"/>
		<rdfs:subClassOf rdf:resource="&java;JavaAPIPart"/>
		<rdfs:seeAlso rdf:resource="&java-se-6;JavaLang"/>
		<rdfs:seeAlso rdf:resource="&java-se-6;JavaNio"/>
		<rdfs:seeAlso rdf:resource="&java-se-6;JavaIo"/>
		<rdfs:seeAlso rdf:resource="&java-se-6;JavaUtil"/>
		<rdfs:comment xml:lang="en">Java API part implementing the java.nio.charset package for Java SE 6</rdfs:comment>
	</owl:Class>
	<owl:Class rdf:about="&java-se-6;JavaNioCharsetSpi">
		<owl:equivalentClass rdf:resource="&j2se-5_0;JavaNioCharsetSpi"/>
		<rdfs:subClassOf rdf:resource="&java;JavaAPIPart"/>
		<rdfs:seeAlso rdf:resource="&java-se-6;JavaLang"/>
		<rdfs:seeAlso rdf:resource="&java-se-6;JavaNioCharset"/>
		<rdfs:seeAlso rdf:resource="&java-se-6;JavaUtil"/>
		<rdfs:comment xml:lang="en">Java API part implementing the java.nio.charset.spi package for Java SE 6</rdfs:comment>
	</owl:Class>
	<owl:Class rdf:about="&java-se-6;JavaUtil">
		<rdfs:subClassOf rdf:resource="&j2se-5_0;JavaUtil"/>
		<rdfs:seeAlso rdf:resource="&java-se-6;JavaLang"/>
		<rdfs:seeAlso rdf:resource="&java-se-6;JavaIo"/>
		<rdfs:seeAlso rdf:resource="&java-se-6;JavaUtilRegex"/>
		<rdfs:seeAlso rdf:resource="&java-se-6;JavaNioChannels"/>
		<rdfs:seeAlso rdf:resource="&java-se-6;JavaSecurity"/>
		<rdfs:seeAlso rdf:resource="&java-se-6;JavaMath"/>
		<rdfs:comment xml:lang="en">Java API part implementing the java.util package for Java SE 6</rdfs:comment>
	</owl:Class>
	<owl:Class rdf:about="&java-se-6;JavaUtilJar">
		<owl:equivalentClass rdf:resource="&j2se-5_0;JavaUtilJar"/>
		<rdfs:subClassOf rdf:resource="&java;JavaAPIPart"/>
		<rdfs:seeAlso rdf:resource="&java-se-6;JavaLang"/>
		<rdfs:seeAlso rdf:resource="&java-se-6;JavaIo"/>
		<rdfs:seeAlso rdf:resource="&java-se-6;JavaBeans"/>
		<rdfs:seeAlso rdf:resource="&java-se-6;JavaUtilZip"/>
		<rdfs:seeAlso rdf:resource="&java-se-6;JavaUtil"/>
		<rdfs:comment xml:lang="en">Java API part implementing the java.util.jar package for Java SE 6</rdfs:comment>
	</owl:Class>
	<owl:Class rdf:about="&java-se-6;JavaUtilSpi">
		<rdfs:subClassOf rdf:resource="&java;JavaAPIPart"/>
		<rdfs:seeAlso rdf:resource="&java-se-6;JavaLang"/>
		<rdfs:seeAlso rdf:resource="&java-se-6;JavaUtil"/>
		<rdfs:comment xml:lang="en">Java API part implementing the java.util.spi package for Java SE 6</rdfs:comment>
	</owl:Class>
	<owl:Class rdf:about="&java-se-6;JavaUtilConcurrent">
		<rdfs:subClassOf rdf:resource="&java;JavaAPIPart"/>
		<rdfs:seeAlso rdf:resource="&java-se-6;JavaLang"/>
		<rdfs:seeAlso rdf:resource="&java-se-6;JavaIo"/>
		<rdfs:seeAlso rdf:resource="&java-se-6;JavaUtil"/>
		<rdfs:seeAlso rdf:resource="&java-se-6;JavaSecurity"/>
		<rdfs:comment xml:lang="en">Java API part implementing the java.util.concurrent package for Java SE 6</rdfs:comment>
	</owl:Class>
	<owl:Class rdf:about="&java-se-6;JavaUtilConcurrentAtomic">
		<rdfs:subClassOf rdf:resource="&j2se-5_0;JavaUtilConcurrentAtomic"/>
		<rdfs:seeAlso rdf:resource="&java-se-6;JavaLang"/>
		<rdfs:seeAlso rdf:resource="&java-se-6;JavaIo"/>
		<rdfs:comment xml:lang="en">Java API part implementing the java.util.concurrent.atomic package for Java SE 6</rdfs:comment>
	</owl:Class>
	<owl:Class rdf:about="&java-se-6;JavaUtilConcurrentLocks">
		<rdfs:subClassOf rdf:resource="&j2se-5_0;JavaUtilConcurrentLocks"/>
		<rdfs:seeAlso rdf:resource="&java-se-6;JavaUtilConcurrent"/>
		<rdfs:seeAlso rdf:resource="&java-se-6;JavaLang"/>
		<rdfs:seeAlso rdf:resource="&java-se-6;JavaIo"/>
		<rdfs:seeAlso rdf:resource="&java-se-6;JavaUtil"/>
		<rdfs:comment xml:lang="en">Java API part implementing the java.util.concurrent.locks package for Java SE 6</rdfs:comment>
	</owl:Class>
	<owl:Class rdf:about="&java-se-6;JavaUtilZip">
		<rdfs:subClassOf rdf:resource="&j2se-5_0;JavaUtilZip"/>
		<rdfs:seeAlso rdf:resource="&java-se-6;JavaLang"/>
		<rdfs:seeAlso rdf:resource="&java-se-6;JavaIo"/>
		<rdfs:seeAlso rdf:resource="&java-se-6;JavaUtil"/>
		<rdfs:comment xml:lang="en">Java API part implementing the java.util.zip package for Java SE 6</rdfs:comment>
	</owl:Class>
	<owl:Class rdf:about="&java-se-6;JavaUtilLogging">
		<rdfs:subClassOf rdf:resource="&j2se-5_0;JavaUtilLogging"/>
		<rdfs:seeAlso rdf:resource="&java-se-6;JavaLang"/>
		<rdfs:seeAlso rdf:resource="&java-se-6;JavaSecurity"/>
		<rdfs:seeAlso rdf:resource="&java-se-6;JavaIo"/>
		<rdfs:seeAlso rdf:resource="&java-se-6;JavaBeans"/>
		<rdfs:seeAlso rdf:resource="&java-se-6;JavaUtil"/>
		<rdfs:comment xml:lang="en">Java API part implementing the java.util.logging package for Java SE 6</rdfs:comment>
	</owl:Class>
	<owl:Class rdf:about="&java-se-6;JavaUtilPrefs">
		<owl:equivalentClass rdf:resource="&j2se-5_0;JavaUtilPrefs"/>
		<rdfs:subClassOf rdf:resource="&java;JavaAPIPart"/>
		<rdfs:seeAlso rdf:resource="&java-se-6;JavaLang"/>
		<rdfs:seeAlso rdf:resource="&java-se-6;JavaIo"/>
		<rdfs:seeAlso rdf:resource="&java-se-6;JavaUtil"/>
		<rdfs:comment xml:lang="en">Java API part implementing the java.util.prefs package for Java SE 6</rdfs:comment>
	</owl:Class>
	<owl:Class rdf:about="&java-se-6;JavaUtilRegex">
		<owl:equivalentClass rdf:resource="&j2se-5_0;JavaUtilRegex"/>
		<rdfs:subClassOf rdf:resource="&java;JavaAPIPart"/>
		<rdfs:seeAlso rdf:resource="&java-se-6;JavaLang"/>
		<rdfs:seeAlso rdf:resource="&java-se-6;JavaIo"/>
		<rdfs:comment xml:lang="en">Java API part implementing the java.util.regex package for Java SE 6</rdfs:comment>
	</owl:Class>
	<owl:Class rdf:about="&java-se-6;JavaApplet">
		<rdfs:subClassOf rdf:resource="&j2se-5_0;JavaApplet"/>
		<rdfs:seeAlso rdf:resource="&java-se-6;JavaAwt"/>
		<rdfs:seeAlso rdf:resource="&java-se-6;JavaLang"/>
		<rdfs:seeAlso rdf:resource="&java-se-6;JavaIo"/>
		<rdfs:seeAlso rdf:resource="&java-se-6;JavaxAccessibility"/>
		<rdfs:seeAlso rdf:resource="&java-se-6;JavaNet"/>
		<rdfs:seeAlso rdf:resource="&java-se-6;JavaUtil"/>
		<rdfs:comment xml:lang="en">Java API part implementing the java.applet package for Java SE 6</rdfs:comment>
	</owl:Class>
	<owl:Class rdf:about="&java-se-6;JavaBeans">
		<rdfs:subClassOf rdf:resource="&j2se-5_0;JavaBeans"/>
		<rdfs:seeAlso rdf:resource="&java-se-6;JavaBeansBeancontext"/>
		<rdfs:seeAlso rdf:resource="&java-se-6;JavaApplet"/>
		<rdfs:seeAlso rdf:resource="&java-se-6;JavaAwt"/>
		<rdfs:seeAlso rdf:resource="&java-se-6;JavaLang"/>
		<rdfs:seeAlso rdf:resource="&java-se-6;JavaIo"/>
		<rdfs:seeAlso rdf:resource="&java-se-6;JavaLangReflect"/>
		<rdfs:seeAlso rdf:resource="&java-se-6;JavaLangAnnotation"/>
		<rdfs:seeAlso rdf:resource="&java-se-6;JavaUtil"/>
		<rdfs:comment xml:lang="en">Java API part implementing the java.beans package for Java SE 6</rdfs:comment>
	</owl:Class>
	<owl:Class rdf:about="&java-se-6;JavaBeansBeancontext">
		<owl:equivalentClass rdf:resource="&j2se-5_0;JavaBeansBeancontext"/>
		<rdfs:subClassOf rdf:resource="&java;JavaAPIPart"/>
		<rdfs:seeAlso rdf:resource="&java-se-6;JavaLang"/>
		<rdfs:seeAlso rdf:resource="&java-se-6;JavaIo"/>
		<rdfs:seeAlso rdf:resource="&java-se-6;JavaBeans"/>
		<rdfs:seeAlso rdf:resource="&java-se-6;JavaUtil"/>
		<rdfs:seeAlso rdf:resource="&java-se-6;JavaAwt"/>
		<rdfs:seeAlso rdf:resource="&java-se-6;JavaNet"/>
		<rdfs:comment xml:lang="en">Java API part implementing the java.beans.beancontext package for Java SE 6</rdfs:comment>
	</owl:Class>
	<owl:Class rdf:about="&java-se-6;JavaText">
		<rdfs:subClassOf rdf:resource="&java;JavaAPIPart"/>
		<rdfs:seeAlso rdf:resource="&java-se-6;JavaLang"/>
		<rdfs:seeAlso rdf:resource="&java-se-6;JavaIo"/>
		<rdfs:seeAlso rdf:resource="&java-se-6;JavaMath"/>
		<rdfs:seeAlso rdf:resource="&java-se-6;JavaUtil"/>
		<rdfs:comment xml:lang="en">Java API part implementing the java.text package for Java SE 6</rdfs:comment>
	</owl:Class>
	<owl:Class rdf:about="&java-se-6;JavaTextSpi">
		<rdfs:subClassOf rdf:resource="&java;JavaAPIPart"/>
		<rdfs:seeAlso rdf:resource="&java-se-6;JavaText"/>
		<rdfs:seeAlso rdf:resource="&java-se-6;JavaUtilSpi"/>
		<rdfs:seeAlso rdf:resource="&java-se-6;JavaUtil"/>
		<rdfs:comment xml:lang="en">Java API part implementing the java.text.spi package for Java SE 6</rdfs:comment>
	</owl:Class>
	<owl:Class rdf:about="&java-se-6;JavaRmi">
		<owl:equivalentClass rdf:resource="&j2se-5_0;JavaRmi"/>
		<rdfs:subClassOf rdf:resource="&java;JavaAPIPart"/>
		<rdfs:seeAlso rdf:resource="&java-se-6;JavaLang"/>
		<rdfs:seeAlso rdf:resource="&java-se-6;JavaIo"/>
		<rdfs:comment xml:lang="en">Java API part implementing the java.rmi package for Java SE 6</rdfs:comment>
	</owl:Class>
	<owl:Class rdf:about="&java-se-6;JavaRmiActivation">
		<owl:equivalentClass rdf:resource="&j2se-5_0;JavaRmiActivation"/>
		<rdfs:subClassOf rdf:resource="&java;JavaAPIPart"/>
		<rdfs:seeAlso rdf:resource="&java-se-6;JavaLang"/>
		<rdfs:seeAlso rdf:resource="&java-se-6;JavaIo"/>
		<rdfs:seeAlso rdf:resource="&java-se-6;JavaRmi"/>
		<rdfs:seeAlso rdf:resource="&java-se-6;JavaUtil"/>
		<rdfs:seeAlso rdf:resource="&java-se-6;JavaRmiServer"/>
		<rdfs:comment xml:lang="en">Java API part implementing the java.rmi.activation package for Java SE 6</rdfs:comment>
	</owl:Class>
	<owl:Class rdf:about="&java-se-6;JavaRmiServer">
		<rdfs:subClassOf rdf:resource="&j2se-5_0;JavaRmiServer"/>
		<rdfs:seeAlso rdf:resource="&java-se-6;JavaLang"/>
		<rdfs:seeAlso rdf:resource="&java-se-6;JavaRmi"/>
		<rdfs:seeAlso rdf:resource="&java-se-6;JavaIo"/>
		<rdfs:seeAlso rdf:resource="&java-se-6;JavaNet"/>
		<rdfs:seeAlso rdf:resource="&java-se-6;JavaLangReflect"/>
		<rdfs:comment xml:lang="en">Java API part implementing the java.rmi.server package for Java SE 6</rdfs:comment>
	</owl:Class>
	<owl:Class rdf:about="&java-se-6;JavaRmiDgc">
		<owl:equivalentClass rdf:resource="&j2se-5_0;JavaRmiDgc"/>
		<rdfs:subClassOf rdf:resource="&java;JavaAPIPart"/>
		<rdfs:seeAlso rdf:resource="&java-se-6;JavaLang"/>
		<rdfs:seeAlso rdf:resource="&java-se-6;JavaRmi"/>
		<rdfs:seeAlso rdf:resource="&java-se-6;JavaIo"/>
		<rdfs:comment xml:lang="en">Java API part implementing the java.rmi.dgc package for Java SE 6</rdfs:comment>
	</owl:Class>
	<owl:Class rdf:about="&java-se-6;JavaRmiRegistry">
		<owl:equivalentClass rdf:resource="&j2se-5_0;JavaRmiRegistry"/>
		<rdfs:subClassOf rdf:resource="&java;JavaAPIPart"/>
		<rdfs:seeAlso rdf:resource="&java-se-6;JavaLang"/>
		<rdfs:seeAlso rdf:resource="&java-se-6;JavaRmi"/>
		<rdfs:seeAlso rdf:resource="&java-se-6;JavaRmiServer"/>
		<rdfs:comment xml:lang="en">Java API part implementing the java.rmi.registry package for Java SE 6</rdfs:comment>
	</owl:Class>
	<owl:Class rdf:about="&java-se-6;JavaSql">
		<rdfs:subClassOf rdf:resource="&j2se-5_0;JavaSql"/>
		<rdfs:seeAlso rdf:resource="&java-se-6;JavaLang"/>
		<rdfs:seeAlso rdf:resource="&java-se-6;JavaIo"/>
		<rdfs:seeAlso rdf:resource="&java-se-6;JavaUtil"/>
		<rdfs:seeAlso rdf:resource="&java-se-6;JavaxXmlTransform"/>
		<rdfs:seeAlso rdf:resource="&java-se-6;JavaSecurity"/>
		<rdfs:seeAlso rdf:resource="&java-se-6;JavaNet"/>
		<rdfs:seeAlso rdf:resource="&java-se-6;JavaMath"/>
		<rdfs:comment xml:lang="en">Java API part implementing the java.sql package for Java SE 6</rdfs:comment>
	</owl:Class>
	<owl:Class rdf:about="&java-se-6;OrgW3cDom">
		<owl:equivalentClass rdf:resource="&j2se-5_0;OrgW3cDom"/>
		<rdfs:subClassOf rdf:resource="&java;JavaAPIPart"/>
		<rdfs:seeAlso rdf:resource="&java-se-6;JavaLang"/>
		<rdfs:comment xml:lang="en">Java API part implementing the org.w3c.dom package for Java SE 6</rdfs:comment>
	</owl:Class>
	<owl:Class rdf:about="&java-se-6;OrgW3cDomLs">
		<owl:equivalentClass rdf:resource="&j2se-5_0;OrgW3cDomLs"/>
		<rdfs:subClassOf rdf:resource="&java;JavaAPIPart"/>
		<rdfs:seeAlso rdf:resource="&java-se-6;OrgW3cDom"/>
		<rdfs:seeAlso rdf:resource="&java-se-6;JavaLang"/>
		<rdfs:seeAlso rdf:resource="&java-se-6;JavaIo"/>
		<rdfs:seeAlso rdf:resource="&java-se-6;OrgW3cDomEvents"/>
		<rdfs:seeAlso rdf:resource="&java-se-6;OrgW3cDomTraversal"/>
		<rdfs:comment xml:lang="en">Java API part implementing the org.w3c.dom.ls package for Java SE 6</rdfs:comment>
	</owl:Class>
	<owl:Class rdf:about="&java-se-6;OrgW3cDomBootstrap">
		<owl:equivalentClass rdf:resource="&j2se-5_0;OrgW3cDomBootstrap"/>
		<rdfs:subClassOf rdf:resource="&java;JavaAPIPart"/>
		<rdfs:seeAlso rdf:resource="&java-se-6;OrgW3cDom"/>
		<rdfs:seeAlso rdf:resource="&java-se-6;JavaLang"/>
		<rdfs:comment xml:lang="en">Java API part implementing the org.w3c.dom.bootstrap package for Java SE 6</rdfs:comment>
	</owl:Class>
	<owl:Class rdf:about="&java-se-6;OrgW3cDomCss">
		<owl:equivalentClass rdf:resource="&j2se-5_0;OrgW3cDomCss"/>
		<rdfs:subClassOf rdf:resource="&java;JavaAPIPart"/>
		<rdfs:seeAlso rdf:resource="&java-se-6;OrgW3cDom"/>
		<rdfs:seeAlso rdf:resource="&java-se-6;JavaLang"/>
		<rdfs:seeAlso rdf:resource="&java-se-6;OrgW3cDomStylesheets"/>
		<rdfs:seeAlso rdf:resource="&java-se-6;OrgW3cDomViews"/>
		<rdfs:comment xml:lang="en">Java API part implementing the org.w3c.dom.css package for Java SE 6</rdfs:comment>
	</owl:Class>
	<owl:Class rdf:about="&java-se-6;OrgW3cDomStylesheets">
		<owl:equivalentClass rdf:resource="&j2se-5_0;OrgW3cDomStylesheets"/>
		<rdfs:subClassOf rdf:resource="&java;JavaAPIPart"/>
		<rdfs:seeAlso rdf:resource="&java-se-6;OrgW3cDom"/>
		<rdfs:seeAlso rdf:resource="&java-se-6;JavaLang"/>
		<rdfs:comment xml:lang="en">Java API part implementing the org.w3c.dom.stylesheets package for Java SE 6</rdfs:comment>
	</owl:Class>
	<owl:Class rdf:about="&java-se-6;OrgW3cDomViews">
		<owl:equivalentClass rdf:resource="&j2se-5_0;OrgW3cDomViews"/>
		<rdfs:subClassOf rdf:resource="&java;JavaAPIPart"/>
		<rdfs:comment xml:lang="en">Java API part implementing the org.w3c.dom.views package for Java SE 6</rdfs:comment>
	</owl:Class>
	<owl:Class rdf:about="&java-se-6;OrgW3cDomEvents">
		<owl:equivalentClass rdf:resource="&j2se-5_0;OrgW3cDomEvents"/>
		<rdfs:subClassOf rdf:resource="&java;JavaAPIPart"/>
		<rdfs:seeAlso rdf:resource="&java-se-6;OrgW3cDom"/>
		<rdfs:seeAlso rdf:resource="&java-se-6;JavaLang"/>
		<rdfs:seeAlso rdf:resource="&java-se-6;OrgW3cDomViews"/>
		<rdfs:comment xml:lang="en">Java API part implementing the org.w3c.dom.events package for Java SE 6</rdfs:comment>
	</owl:Class>
	<owl:Class rdf:about="&java-se-6;OrgW3cDomHtml">
		<owl:equivalentClass rdf:resource="&j2se-5_0;OrgW3cDomHtml"/>
		<rdfs:subClassOf rdf:resource="&java;JavaAPIPart"/>
		<rdfs:seeAlso rdf:resource="&java-se-6;OrgW3cDom"/>
		<rdfs:seeAlso rdf:resource="&java-se-6;JavaLang"/>
		<rdfs:comment xml:lang="en">Java API part implementing the org.w3c.dom.html package for Java SE 6</rdfs:comment>
	</owl:Class>
	<owl:Class rdf:about="&java-se-6;OrgW3cDomTraversal">
		<owl:equivalentClass rdf:resource="&j2se-5_0;OrgW3cDomTraversal"/>
		<rdfs:subClassOf rdf:resource="&java;JavaAPIPart"/>
		<rdfs:seeAlso rdf:resource="&java-se-6;OrgW3cDom"/>
		<rdfs:comment xml:lang="en">Java API part implementing the org.w3c.dom.traversal package for Java SE 6</rdfs:comment>
	</owl:Class>
	<owl:Class rdf:about="&java-se-6;OrgW3cDomRanges">
		<owl:equivalentClass rdf:resource="&j2se-5_0;OrgW3cDomRanges"/>
		<rdfs:subClassOf rdf:resource="&java;JavaAPIPart"/>
		<rdfs:seeAlso rdf:resource="&java-se-6;OrgW3cDom"/>
		<rdfs:seeAlso rdf:resource="&java-se-6;JavaLang"/>
		<rdfs:comment xml:lang="en">Java API part implementing the org.w3c.dom.ranges package for Java SE 6</rdfs:comment>
	</owl:Class>
	<owl:Class rdf:about="&java-se-6;OrgW3cDomXpath">
		<rdfs:subClassOf rdf:resource="&java;JavaAPIPart"/>
		<rdfs:seeAlso rdf:resource="&java-se-6;OrgW3cDom"/>
		<rdfs:seeAlso rdf:resource="&java-se-6;JavaLang"/>
		<rdfs:comment xml:lang="en">Java API part implementing the org.w3c.dom.xpath package for Java SE 6</rdfs:comment>
	</owl:Class>
	<owl:Class rdf:about="&java-se-6;OrgOmgCORBA_2_3">
		<owl:equivalentClass rdf:resource="&j2se-5_0;OrgOmgCORBA_2_3"/>
		<rdfs:subClassOf rdf:resource="&java;JavaAPIPart"/>
		<rdfs:seeAlso rdf:resource="&java-se-6;OrgOmgCORBAPortable"/>
		<rdfs:seeAlso rdf:resource="&java-se-6;OrgOmgCORBA"/>
		<rdfs:seeAlso rdf:resource="&java-se-6;JavaLang"/>
		<rdfs:comment xml:lang="en">Java API part implementing the org.omg.CORBA_2_3 package for Java SE 6</rdfs:comment>
	</owl:Class>
	<owl:Class rdf:about="&java-se-6;OrgOmgCORBA_2_3Portable">
		<owl:equivalentClass rdf:resource="&j2se-5_0;OrgOmgCORBA_2_3Portable"/>
		<rdfs:subClassOf rdf:resource="&java;JavaAPIPart"/>
		<rdfs:seeAlso rdf:resource="&java-se-6;OrgOmgCORBAPortable"/>
		<rdfs:seeAlso rdf:resource="&java-se-6;OrgOmgCORBA"/>
		<rdfs:seeAlso rdf:resource="&java-se-6;JavaLang"/>
		<rdfs:seeAlso rdf:resource="&java-se-6;JavaIo"/>
		<rdfs:comment xml:lang="en">Java API part implementing the org.omg.CORBA_2_3.portable package for Java SE 6</rdfs:comment>
	</owl:Class>
	<owl:Class rdf:about="&java-se-6;OrgOmgCORBA">
		<owl:equivalentClass rdf:resource="&j2se-5_0;OrgOmgCORBA"/>
		<rdfs:subClassOf rdf:resource="&java;JavaAPIPart"/>
		<rdfs:seeAlso rdf:resource="&java-se-6;OrgOmgCORBAPortable"/>
		<rdfs:seeAlso rdf:resource="&java-se-6;JavaApplet"/>
		<rdfs:seeAlso rdf:resource="&java-se-6;JavaLang"/>
		<rdfs:seeAlso rdf:resource="&java-se-6;JavaIo"/>
		<rdfs:seeAlso rdf:resource="&java-se-6;JavaMath"/>
		<rdfs:seeAlso rdf:resource="&java-se-6;JavaUtil"/>
		<rdfs:comment xml:lang="en">Java API part implementing the org.omg.CORBA package for Java SE 6</rdfs:comment>
	</owl:Class>
	<owl:Class rdf:about="&java-se-6;OrgOmgCORBAPortable">
		<owl:equivalentClass rdf:resource="&j2se-5_0;OrgOmgCORBAPortable"/>
		<rdfs:subClassOf rdf:resource="&java;JavaAPIPart"/>
		<rdfs:seeAlso rdf:resource="&java-se-6;JavaLang"/>
		<rdfs:seeAlso rdf:resource="&java-se-6;JavaIo"/>
		<rdfs:seeAlso rdf:resource="&java-se-6;OrgOmgCORBA_2_3Portable"/>
		<rdfs:seeAlso rdf:resource="&java-se-6;OrgOmgCORBA"/>
		<rdfs:seeAlso rdf:resource="&java-se-6;JavaMath"/>
		<rdfs:comment xml:lang="en">Java API part implementing the org.omg.CORBA.portable package for Java SE 6</rdfs:comment>
	</owl:Class>
	<owl:Class rdf:about="&java-se-6;OrgOmgCORBADynAnyPackage">
		<owl:equivalentClass rdf:resource="&j2se-5_0;OrgOmgCORBADynAnyPackage"/>
		<rdfs:subClassOf rdf:resource="&java;JavaAPIPart"/>
		<rdfs:seeAlso rdf:resource="&java-se-6;OrgOmgCORBA"/>
		<rdfs:seeAlso rdf:resource="&java-se-6;JavaLang"/>
		<rdfs:comment xml:lang="en">Java API part implementing the org.omg.CORBA.DynAnyPackage package for Java SE 6</rdfs:comment>
	</owl:Class>
	<owl:Class rdf:about="&java-se-6;OrgOmgCORBAORBPackage">
		<owl:equivalentClass rdf:resource="&j2se-5_0;OrgOmgCORBAORBPackage"/>
		<rdfs:subClassOf rdf:resource="&java;JavaAPIPart"/>
		<rdfs:seeAlso rdf:resource="&java-se-6;OrgOmgCORBA"/>
		<rdfs:seeAlso rdf:resource="&java-se-6;JavaLang"/>
		<rdfs:comment xml:lang="en">Java API part implementing the org.omg.CORBA.ORBPackage package for Java SE 6</rdfs:comment>
	</owl:Class>
	<owl:Class rdf:about="&java-se-6;OrgOmgCORBATypeCodePackage">
		<owl:equivalentClass rdf:resource="&j2se-5_0;OrgOmgCORBATypeCodePackage"/>
		<rdfs:subClassOf rdf:resource="&java;JavaAPIPart"/>
		<rdfs:seeAlso rdf:resource="&java-se-6;OrgOmgCORBA"/>
		<rdfs:seeAlso rdf:resource="&java-se-6;JavaLang"/>
		<rdfs:comment xml:lang="en">Java API part implementing the org.omg.CORBA.TypeCodePackage package for Java SE 6</rdfs:comment>
	</owl:Class>
	<owl:Class rdf:about="&java-se-6;OrgOmgSendingContext">
		<owl:equivalentClass rdf:resource="&j2se-5_0;OrgOmgSendingContext"/>
		<rdfs:subClassOf rdf:resource="&java;JavaAPIPart"/>
		<rdfs:seeAlso rdf:resource="&java-se-6;OrgOmgCORBAPortable"/>
		<rdfs:seeAlso rdf:resource="&java-se-6;OrgOmgCORBA"/>
		<rdfs:comment xml:lang="en">Java API part implementing the org.omg.SendingContext package for Java SE 6</rdfs:comment>
	</owl:Class>
	<owl:Class rdf:about="&java-se-6;OrgOmgCosNaming">
		<owl:equivalentClass rdf:resource="&j2se-5_0;OrgOmgCosNaming"/>
		<rdfs:subClassOf rdf:resource="&java;JavaAPIPart"/>
		<rdfs:seeAlso rdf:resource="&java-se-6;OrgOmgCORBAPortable"/>
		<rdfs:seeAlso rdf:resource="&java-se-6;JavaLang"/>
		<rdfs:seeAlso rdf:resource="&java-se-6;OrgOmgPortableServer"/>
		<rdfs:seeAlso rdf:resource="&java-se-6;OrgOmgCORBA"/>
		<rdfs:comment xml:lang="en">Java API part implementing the org.omg.CosNaming package for Java SE 6</rdfs:comment>
	</owl:Class>
	<owl:Class rdf:about="&java-se-6;OrgOmgCosNamingNamingContextExtPackage">
		<owl:equivalentClass rdf:resource="&j2se-5_0;OrgOmgCosNamingNamingContextExtPackage"/>
		<rdfs:subClassOf rdf:resource="&java;JavaAPIPart"/>
		<rdfs:seeAlso rdf:resource="&java-se-6;OrgOmgCORBAPortable"/>
		<rdfs:seeAlso rdf:resource="&java-se-6;OrgOmgCORBA"/>
		<rdfs:seeAlso rdf:resource="&java-se-6;JavaLang"/>
		<rdfs:comment xml:lang="en">Java API part implementing the org.omg.CosNaming.NamingContextExtPackage package for Java SE 6</rdfs:comment>
	</owl:Class>
	<owl:Class rdf:about="&java-se-6;OrgOmgCosNamingNamingContextPackage">
		<owl:equivalentClass rdf:resource="&j2se-5_0;OrgOmgCosNamingNamingContextPackage"/>
		<rdfs:subClassOf rdf:resource="&java;JavaAPIPart"/>
		<rdfs:seeAlso rdf:resource="&java-se-6;OrgOmgCORBAPortable"/>
		<rdfs:seeAlso rdf:resource="&java-se-6;OrgOmgCORBA"/>
		<rdfs:seeAlso rdf:resource="&java-se-6;JavaLang"/>
		<rdfs:seeAlso rdf:resource="&java-se-6;OrgOmgCosNaming"/>
		<rdfs:comment xml:lang="en">Java API part implementing the org.omg.CosNaming.NamingContextPackage package for Java SE 6</rdfs:comment>
	</owl:Class>
	<owl:Class rdf:about="&java-se-6;OrgOmgPortableServer">
		<owl:equivalentClass rdf:resource="&j2se-5_0;OrgOmgPortableServer"/>
		<rdfs:subClassOf rdf:resource="&java;JavaAPIPart"/>
		<rdfs:seeAlso rdf:resource="&java-se-6;OrgOmgCORBAPortable"/>
		<rdfs:seeAlso rdf:resource="&java-se-6;OrgOmgPortableServerPOAManagerPackage"/>
		<rdfs:seeAlso rdf:resource="&java-se-6;JavaLang"/>
		<rdfs:seeAlso rdf:resource="&java-se-6;OrgOmgPortableServerServantLocatorPackage"/>
		<rdfs:seeAlso rdf:resource="&java-se-6;OrgOmgCORBA"/>
		<rdfs:seeAlso rdf:resource="&java-se-6;OrgOmgPortableServerPortable"/>
		<rdfs:comment xml:lang="en">Java API part implementing the org.omg.PortableServer package for Java SE 6</rdfs:comment>
	</owl:Class>
	<owl:Class rdf:about="&java-se-6;OrgOmgPortableServerCurrentPackage">
		<owl:equivalentClass rdf:resource="&j2se-5_0;OrgOmgPortableServerCurrentPackage"/>
		<rdfs:subClassOf rdf:resource="&java;JavaAPIPart"/>
		<rdfs:seeAlso rdf:resource="&java-se-6;OrgOmgCORBAPortable"/>
		<rdfs:seeAlso rdf:resource="&java-se-6;OrgOmgCORBA"/>
		<rdfs:seeAlso rdf:resource="&java-se-6;JavaLang"/>
		<rdfs:comment xml:lang="en">Java API part implementing the org.omg.PortableServer.CurrentPackage package for Java SE 6</rdfs:comment>
	</owl:Class>
	<owl:Class rdf:about="&java-se-6;OrgOmgPortableServerPOAManagerPackage">
		<owl:equivalentClass rdf:resource="&j2se-5_0;OrgOmgPortableServerPOAManagerPackage"/>
		<rdfs:subClassOf rdf:resource="&java;JavaAPIPart"/>
		<rdfs:seeAlso rdf:resource="&java-se-6;OrgOmgCORBAPortable"/>
		<rdfs:seeAlso rdf:resource="&java-se-6;OrgOmgCORBA"/>
		<rdfs:seeAlso rdf:resource="&java-se-6;JavaLang"/>
		<rdfs:comment xml:lang="en">Java API part implementing the org.omg.PortableServer.POAManagerPackage package for Java SE 6</rdfs:comment>
	</owl:Class>
	<owl:Class rdf:about="&java-se-6;OrgOmgPortableServerPOAPackage">
		<owl:equivalentClass rdf:resource="&j2se-5_0;OrgOmgPortableServerPOAPackage"/>
		<rdfs:subClassOf rdf:resource="&java;JavaAPIPart"/>
		<rdfs:seeAlso rdf:resource="&java-se-6;OrgOmgCORBAPortable"/>
		<rdfs:seeAlso rdf:resource="&java-se-6;OrgOmgCORBA"/>
		<rdfs:seeAlso rdf:resource="&java-se-6;JavaLang"/>
		<rdfs:comment xml:lang="en">Java API part implementing the org.omg.PortableServer.POAPackage package for Java SE 6</rdfs:comment>
	</owl:Class>
	<owl:Class rdf:about="&java-se-6;OrgOmgPortableServerPortable">
		<owl:equivalentClass rdf:resource="&j2se-5_0;OrgOmgPortableServerPortable"/>
		<rdfs:subClassOf rdf:resource="&java;JavaAPIPart"/>
		<rdfs:seeAlso rdf:resource="&java-se-6;OrgOmgCORBA"/>
		<rdfs:seeAlso rdf:resource="&java-se-6;JavaLang"/>
		<rdfs:seeAlso rdf:resource="&java-se-6;OrgOmgPortableServer"/>
		<rdfs:comment xml:lang="en">Java API part implementing the org.omg.PortableServer.portable package for Java SE 6</rdfs:comment>
	</owl:Class>
	<owl:Class rdf:about="&java-se-6;OrgOmgPortableServerServantLocatorPackage">
		<owl:equivalentClass rdf:resource="&j2se-5_0;OrgOmgPortableServerServantLocatorPackage"/>
		<rdfs:subClassOf rdf:resource="&java;JavaAPIPart"/>
		<rdfs:seeAlso rdf:resource="&java-se-6;OrgOmgCORBAPortable"/>
		<rdfs:seeAlso rdf:resource="&java-se-6;OrgOmgCORBA"/>
		<rdfs:seeAlso rdf:resource="&java-se-6;JavaLang"/>
		<rdfs:comment xml:lang="en">Java API part implementing the org.omg.PortableServer.ServantLocatorPackage package for Java SE 6</rdfs:comment>
	</owl:Class>
	<owl:Class rdf:about="&java-se-6;OrgOmgDynamic">
		<owl:equivalentClass rdf:resource="&j2se-5_0;OrgOmgDynamic"/>
		<rdfs:subClassOf rdf:resource="&java;JavaAPIPart"/>
		<rdfs:seeAlso rdf:resource="&java-se-6;OrgOmgCORBAPortable"/>
		<rdfs:seeAlso rdf:resource="&java-se-6;OrgOmgCORBA"/>
		<rdfs:seeAlso rdf:resource="&java-se-6;JavaLang"/>
		<rdfs:comment xml:lang="en">Java API part implementing the org.omg.Dynamic package for Java SE 6</rdfs:comment>
	</owl:Class>
	<owl:Class rdf:about="&java-se-6;OrgOmgDynamicAny">
		<owl:equivalentClass rdf:resource="&j2se-5_0;OrgOmgDynamicAny"/>
		<rdfs:subClassOf rdf:resource="&java;JavaAPIPart"/>
		<rdfs:seeAlso rdf:resource="&java-se-6;OrgOmgCORBAPortable"/>
		<rdfs:seeAlso rdf:resource="&java-se-6;JavaLang"/>
		<rdfs:seeAlso rdf:resource="&java-se-6;JavaIo"/>
		<rdfs:seeAlso rdf:resource="&java-se-6;OrgOmgCORBA"/>
		<rdfs:comment xml:lang="en">Java API part implementing the org.omg.DynamicAny package for Java SE 6</rdfs:comment>
	</owl:Class>
	<owl:Class rdf:about="&java-se-6;OrgOmgDynamicAnyDynAnyFactoryPackage">
		<owl:equivalentClass rdf:resource="&j2se-5_0;OrgOmgDynamicAnyDynAnyFactoryPackage"/>
		<rdfs:subClassOf rdf:resource="&java;JavaAPIPart"/>
		<rdfs:seeAlso rdf:resource="&java-se-6;OrgOmgCORBAPortable"/>
		<rdfs:seeAlso rdf:resource="&java-se-6;OrgOmgCORBA"/>
		<rdfs:seeAlso rdf:resource="&java-se-6;JavaLang"/>
		<rdfs:comment xml:lang="en">Java API part implementing the org.omg.DynamicAny.DynAnyFactoryPackage package for Java SE 6</rdfs:comment>
	</owl:Class>
	<owl:Class rdf:about="&java-se-6;OrgOmgDynamicAnyDynAnyPackage">
		<owl:equivalentClass rdf:resource="&j2se-5_0;OrgOmgDynamicAnyDynAnyPackage"/>
		<rdfs:subClassOf rdf:resource="&java;JavaAPIPart"/>
		<rdfs:seeAlso rdf:resource="&java-se-6;OrgOmgCORBAPortable"/>
		<rdfs:seeAlso rdf:resource="&java-se-6;OrgOmgCORBA"/>
		<rdfs:seeAlso rdf:resource="&java-se-6;JavaLang"/>
		<rdfs:comment xml:lang="en">Java API part implementing the org.omg.DynamicAny.DynAnyPackage package for Java SE 6</rdfs:comment>
	</owl:Class>
	<owl:Class rdf:about="&java-se-6;OrgOmgIOP">
		<owl:equivalentClass rdf:resource="&j2se-5_0;OrgOmgIOP"/>
		<rdfs:subClassOf rdf:resource="&java;JavaAPIPart"/>
		<rdfs:seeAlso rdf:resource="&java-se-6;OrgOmgCORBAPortable"/>
		<rdfs:seeAlso rdf:resource="&java-se-6;OrgOmgCORBA"/>
		<rdfs:seeAlso rdf:resource="&java-se-6;JavaLang"/>
		<rdfs:comment xml:lang="en">Java API part implementing the org.omg.IOP package for Java SE 6</rdfs:comment>
	</owl:Class>
	<owl:Class rdf:about="&java-se-6;OrgOmgIOPCodecFactoryPackage">
		<owl:equivalentClass rdf:resource="&j2se-5_0;OrgOmgIOPCodecFactoryPackage"/>
		<rdfs:subClassOf rdf:resource="&java;JavaAPIPart"/>
		<rdfs:seeAlso rdf:resource="&java-se-6;OrgOmgCORBAPortable"/>
		<rdfs:seeAlso rdf:resource="&java-se-6;OrgOmgCORBA"/>
		<rdfs:seeAlso rdf:resource="&java-se-6;JavaLang"/>
		<rdfs:comment xml:lang="en">Java API part implementing the org.omg.IOP.CodecFactoryPackage package for Java SE 6</rdfs:comment>
	</owl:Class>
	<owl:Class rdf:about="&java-se-6;OrgOmgIOPCodecPackage">
		<owl:equivalentClass rdf:resource="&j2se-5_0;OrgOmgIOPCodecPackage"/>
		<rdfs:subClassOf rdf:resource="&java;JavaAPIPart"/>
		<rdfs:seeAlso rdf:resource="&java-se-6;OrgOmgCORBAPortable"/>
		<rdfs:seeAlso rdf:resource="&java-se-6;OrgOmgCORBA"/>
		<rdfs:seeAlso rdf:resource="&java-se-6;JavaLang"/>
		<rdfs:comment xml:lang="en">Java API part implementing the org.omg.IOP.CodecPackage package for Java SE 6</rdfs:comment>
	</owl:Class>
	<owl:Class rdf:about="&java-se-6;OrgOmgMessaging">
		<owl:equivalentClass rdf:resource="&j2se-5_0;OrgOmgMessaging"/>
		<rdfs:subClassOf rdf:resource="&java;JavaAPIPart"/>
		<rdfs:seeAlso rdf:resource="&java-se-6;OrgOmgCORBAPortable"/>
		<rdfs:seeAlso rdf:resource="&java-se-6;OrgOmgCORBA"/>
		<rdfs:seeAlso rdf:resource="&java-se-6;JavaLang"/>
		<rdfs:comment xml:lang="en">Java API part implementing the org.omg.Messaging package for Java SE 6</rdfs:comment>
	</owl:Class>
	<owl:Class rdf:about="&java-se-6;OrgOmgPortableInterceptor">
		<owl:equivalentClass rdf:resource="&j2se-5_0;OrgOmgPortableInterceptor"/>
		<rdfs:subClassOf rdf:resource="&java;JavaAPIPart"/>
		<rdfs:seeAlso rdf:resource="&java-se-6;OrgOmgCORBAPortable"/>
		<rdfs:seeAlso rdf:resource="&java-se-6;JavaLang"/>
		<rdfs:seeAlso rdf:resource="&java-se-6;OrgOmgIOP"/>
		<rdfs:seeAlso rdf:resource="&java-se-6;OrgOmgCORBA"/>
		<rdfs:comment xml:lang="en">Java API part implementing the org.omg.PortableInterceptor package for Java SE 6</rdfs:comment>
	</owl:Class>
	<owl:Class rdf:about="&java-se-6;OrgOmgPortableInterceptorORBInitInfoPackage">
		<owl:equivalentClass rdf:resource="&j2se-5_0;OrgOmgPortableInterceptorORBInitInfoPackage"/>
		<rdfs:subClassOf rdf:resource="&java;JavaAPIPart"/>
		<rdfs:seeAlso rdf:resource="&java-se-6;OrgOmgCORBAPortable"/>
		<rdfs:seeAlso rdf:resource="&java-se-6;OrgOmgCORBA"/>
		<rdfs:seeAlso rdf:resource="&java-se-6;JavaLang"/>
		<rdfs:comment xml:lang="en">Java API part implementing the org.omg.PortableInterceptor.ORBInitInfoPackage package for Java SE 6</rdfs:comment>
	</owl:Class>
	<owl:Class rdf:about="&java-se-6;OrgOmgStubJavaRmi">
		<owl:equivalentClass rdf:resource="&j2se-5_0;OrgOmgStubJavaRmi"/>
		<rdfs:subClassOf rdf:resource="&java;JavaAPIPart"/>
		<rdfs:seeAlso rdf:resource="&java-se-6;JavaxRmiCORBA"/>
		<rdfs:seeAlso rdf:resource="&java-se-6;JavaRmi"/>
		<rdfs:comment xml:lang="en">Java API part implementing the org.omg.stub.java.rmi package for Java SE 6</rdfs:comment>
	</owl:Class>
	<owl:Class rdf:about="&java-se-6;OrgOmgStubJavaxManagementRemoteRmi">
		<owl:equivalentClass rdf:resource="&j2se-5_0;OrgOmgStubJavaxManagementRemoteRmi"/>
		<rdfs:subClassOf rdf:resource="&java;JavaAPIPart"/>
		<rdfs:seeAlso rdf:resource="&java-se-6;OrgOmgCORBAPortable"/>
		<rdfs:seeAlso rdf:resource="&java-se-6;JavaxManagement"/>
		<rdfs:seeAlso rdf:resource="&java-se-6;JavaLang"/>
		<rdfs:seeAlso rdf:resource="&java-se-6;JavaRmi"/>
		<rdfs:seeAlso rdf:resource="&java-se-6;OrgOmgCORBA_2_3Portable"/>
		<rdfs:seeAlso rdf:resource="&java-se-6;JavaxManagementRemote"/>
		<rdfs:seeAlso rdf:resource="&java-se-6;OrgOmgCORBA"/>
		<rdfs:seeAlso rdf:resource="&java-se-6;JavaxRmiCORBA"/>
		<rdfs:seeAlso rdf:resource="&java-se-6;JavaxManagementRemoteRmi"/>
		<rdfs:seeAlso rdf:resource="&java-se-6;JavaxSecurityAuth"/>
		<rdfs:seeAlso rdf:resource="&java-se-6;JavaUtil"/>
		<rdfs:comment xml:lang="en">Java API part implementing the org.omg.stub.javax.management.remote.rmi package for Java SE 6</rdfs:comment>
	</owl:Class>
	<owl:Class rdf:about="&java-se-6;OrgXmlSax">
		<owl:equivalentClass rdf:resource="&j2se-5_0;OrgXmlSax"/>
		<rdfs:subClassOf rdf:resource="&java;JavaAPIPart"/>
		<rdfs:seeAlso rdf:resource="&java-se-6;JavaLang"/>
		<rdfs:seeAlso rdf:resource="&java-se-6;JavaIo"/>
		<rdfs:seeAlso rdf:resource="&java-se-6;JavaUtil"/>
		<rdfs:comment xml:lang="en">Java API part implementing the org.xml.sax package for Java SE 6</rdfs:comment>
	</owl:Class>
	<owl:Class rdf:about="&java-se-6;OrgXmlSaxHelpers">
		<owl:equivalentClass rdf:resource="&j2se-5_0;OrgXmlSaxHelpers"/>
		<rdfs:subClassOf rdf:resource="&java;JavaAPIPart"/>
		<rdfs:seeAlso rdf:resource="&java-se-6;JavaLang"/>
		<rdfs:seeAlso rdf:resource="&java-se-6;OrgXmlSax"/>
		<rdfs:seeAlso rdf:resource="&java-se-6;JavaUtil"/>
		<rdfs:comment xml:lang="en">Java API part implementing the org.xml.sax.helpers package for Java SE 6</rdfs:comment>
	</owl:Class>
	<owl:Class rdf:about="&java-se-6;OrgXmlSaxExt">
		<owl:equivalentClass rdf:resource="&j2se-5_0;OrgXmlSaxExt"/>
		<rdfs:subClassOf rdf:resource="&java;JavaAPIPart"/>
		<rdfs:seeAlso rdf:resource="&java-se-6;OrgXmlSaxHelpers"/>
		<rdfs:seeAlso rdf:resource="&java-se-6;JavaLang"/>
		<rdfs:seeAlso rdf:resource="&java-se-6;OrgXmlSax"/>
		<rdfs:comment xml:lang="en">Java API part implementing the org.xml.sax.ext package for Java SE 6</rdfs:comment>
	</owl:Class>
	<owl:Class rdf:about="&java-se-6;OrgIetfJgss">
		<owl:equivalentClass rdf:resource="&j2se-5_0;OrgIetfJgss"/>
		<rdfs:subClassOf rdf:resource="&java;JavaAPIPart"/>
		<rdfs:seeAlso rdf:resource="&java-se-6;JavaNet"/>
		<rdfs:seeAlso rdf:resource="&java-se-6;JavaLang"/>
		<rdfs:seeAlso rdf:resource="&java-se-6;JavaSecurity"/>
		<rdfs:seeAlso rdf:resource="&java-se-6;JavaIo"/>
		<rdfs:comment xml:lang="en">Java API part implementing the org.ietf.jgss package for Java SE 6</rdfs:comment>
	</owl:Class>
	<owl:Class rdf:about="&java-se-6;JavaxJnlpAPI">
		<rdfs:subClassOf rdf:resource="&java;JavaAPI"/>
		<rdfs:comment xml:lang="en">JavaLibrary implementing the javax.jnlp package for Java SE 6</rdfs:comment>
		<rdfs:comment xml:lang="OWLManchester">platform:comprisesInterfacePart some JavaxJnlp</rdfs:comment>
	</owl:Class>
	<owl:Class rdf:about="&java-se-6;JavaxCryptoAPI">
		<owl:equivalentClass rdf:resource="&j2se-5_0;JavaxCryptoAPI"/>
		<rdfs:subClassOf rdf:resource="&java;JavaAPI"/>
		<rdfs:comment xml:lang="en">JavaLibrary implementing the javax.crypto package for Java SE 6</rdfs:comment>
		<rdfs:comment xml:lang="OWLManchester">platform:comprisesInterfacePart some JavaxCrypto</rdfs:comment>
	</owl:Class>
	<owl:Class rdf:about="&java-se-6;JavaxCryptoInterfacesAPI">
		<owl:equivalentClass rdf:resource="&j2se-5_0;JavaxCryptoInterfacesAPI"/>
		<rdfs:subClassOf rdf:resource="&java;JavaAPI"/>
		<rdfs:comment xml:lang="en">JavaLibrary implementing the javax.crypto.interfaces package for Java SE 6</rdfs:comment>
		<rdfs:comment xml:lang="OWLManchester">platform:comprisesInterfacePart some JavaxCryptoInterfaces</rdfs:comment>
	</owl:Class>
	<owl:Class rdf:about="&java-se-6;JavaxCryptoSpecAPI">
		<owl:equivalentClass rdf:resource="&j2se-5_0;JavaxCryptoSpecAPI"/>
		<rdfs:subClassOf rdf:resource="&java;JavaAPI"/>
		<rdfs:comment xml:lang="en">JavaLibrary implementing the javax.crypto.spec package for Java SE 6</rdfs:comment>
		<rdfs:comment xml:lang="OWLManchester">platform:comprisesInterfacePart some JavaxCryptoSpec</rdfs:comment>
	</owl:Class>
	<owl:Class rdf:about="&java-se-6;JavaxNetAPI">
		<owl:equivalentClass rdf:resource="&j2se-5_0;JavaxNetAPI"/>
		<rdfs:subClassOf rdf:resource="&java;JavaAPI"/>
		<rdfs:comment xml:lang="en">JavaLibrary implementing the javax.net package for Java SE 6</rdfs:comment>
		<rdfs:comment xml:lang="OWLManchester">platform:comprisesInterfacePart some JavaxNet</rdfs:comment>
	</owl:Class>
	<owl:Class rdf:about="&java-se-6;JavaxNetSslAPI">
		<rdfs:subClassOf rdf:resource="&j2se-5_0;JavaxNetSslAPI"/>
		<rdfs:comment xml:lang="en">JavaLibrary implementing the javax.net.ssl package for Java SE 6</rdfs:comment>
		<rdfs:comment xml:lang="OWLManchester">platform:comprisesInterfacePart some JavaxNetSsl</rdfs:comment>
	</owl:Class>
	<owl:Class rdf:about="&java-se-6;JavaxSecurityCertAPI">
		<owl:equivalentClass rdf:resource="&j2se-5_0;JavaxSecurityCertAPI"/>
		<rdfs:subClassOf rdf:resource="&java;JavaAPI"/>
		<rdfs:comment xml:lang="en">JavaLibrary implementing the javax.security.cert package for Java SE 6</rdfs:comment>
		<rdfs:comment xml:lang="OWLManchester">platform:comprisesInterfacePart some JavaxSecurityCert</rdfs:comment>
	</owl:Class>
	<owl:Class rdf:about="&java-se-6;JavaxSecurityAuthAPI">
		<owl:equivalentClass rdf:resource="&j2se-5_0;JavaxSecurityAuthAPI"/>
		<rdfs:subClassOf rdf:resource="&java;JavaAPI"/>
		<rdfs:comment xml:lang="en">JavaLibrary implementing the javax.security.auth package for Java SE 6</rdfs:comment>
		<rdfs:comment xml:lang="OWLManchester">platform:comprisesInterfacePart some JavaxSecurityAuth</rdfs:comment>
	</owl:Class>
	<owl:Class rdf:about="&java-se-6;JavaxSecurityAuthCallbackAPI">
		<owl:equivalentClass rdf:resource="&j2se-5_0;JavaxSecurityAuthCallbackAPI"/>
		<rdfs:subClassOf rdf:resource="&java;JavaAPI"/>
		<rdfs:comment xml:lang="en">JavaLibrary implementing the javax.security.auth.callback package for Java SE 6</rdfs:comment>
		<rdfs:comment xml:lang="OWLManchester">platform:comprisesInterfacePart some JavaxSecurityAuthCallback</rdfs:comment>
	</owl:Class>
	<owl:Class rdf:about="&java-se-6;JavaxSecurityAuthLoginAPI">
		<rdfs:subClassOf rdf:resource="&j2se-5_0;JavaxSecurityAuthLoginAPI"/>
		<rdfs:comment xml:lang="en">JavaLibrary implementing the javax.security.auth.login package for Java SE 6</rdfs:comment>
		<rdfs:comment xml:lang="OWLManchester">platform:comprisesInterfacePart some JavaxSecurityAuthLogin</rdfs:comment>
	</owl:Class>
	<owl:Class rdf:about="&java-se-6;JavaxSecurityAuthX500API">
		<rdfs:subClassOf rdf:resource="&j2se-5_0;JavaxSecurityAuthX500API"/>
		<rdfs:comment xml:lang="en">JavaLibrary implementing the javax.security.auth.x500 package for Java SE 6</rdfs:comment>
		<rdfs:comment xml:lang="OWLManchester">platform:comprisesInterfacePart some JavaxSecurityAuthX500</rdfs:comment>
	</owl:Class>
	<owl:Class rdf:about="&java-se-6;JavaxSecurityAuthKerberosAPI">
		<owl:equivalentClass rdf:resource="&j2se-5_0;JavaxSecurityAuthKerberosAPI"/>
		<rdfs:subClassOf rdf:resource="&java;JavaAPI"/>
		<rdfs:comment xml:lang="en">JavaLibrary implementing the javax.security.auth.kerberos package for Java SE 6</rdfs:comment>
		<rdfs:comment xml:lang="OWLManchester">platform:comprisesInterfacePart some JavaxSecurityAuthKerberos</rdfs:comment>
	</owl:Class>
	<owl:Class rdf:about="&java-se-6;JavaxSecurityAuthSpiAPI">
		<owl:equivalentClass rdf:resource="&j2se-5_0;JavaxSecurityAuthSpiAPI"/>
		<rdfs:subClassOf rdf:resource="&java;JavaAPI"/>
		<rdfs:comment xml:lang="en">JavaLibrary implementing the javax.security.auth.spi package for Java SE 6</rdfs:comment>
		<rdfs:comment xml:lang="OWLManchester">platform:comprisesInterfacePart some JavaxSecurityAuthSpi</rdfs:comment>
	</owl:Class>
	<owl:Class rdf:about="&java-se-6;JavaxSecuritySaslAPI">
		<rdfs:subClassOf rdf:resource="&j2se-5_0;JavaxSecuritySaslAPI"/>
		<rdfs:comment xml:lang="en">JavaLibrary implementing the javax.security.sasl package for Java SE 6</rdfs:comment>
		<rdfs:comment xml:lang="OWLManchester">platform:comprisesInterfacePart some JavaxSecuritySasl</rdfs:comment>
	</owl:Class>
	<owl:Class rdf:about="&java-se-6;JavaxAccessibilityAPI">
		<rdfs:subClassOf rdf:resource="&j2se-5_0;JavaxAccessibilityAPI"/>
		<rdfs:comment xml:lang="en">JavaLibrary implementing the javax.accessibility package for Java SE 6</rdfs:comment>
		<rdfs:comment xml:lang="OWLManchester">platform:comprisesInterfacePart some JavaxAccessibility</rdfs:comment>
	</owl:Class>
	<owl:Class rdf:about="&java-se-6;JavaxSwingAPI">
		<rdfs:subClassOf rdf:resource="&j2se-5_0;JavaxSwingAPI"/>
		<rdfs:comment xml:lang="en">JavaLibrary implementing the javax.swing package for Java SE 6</rdfs:comment>
		<rdfs:comment xml:lang="OWLManchester">platform:comprisesInterfacePart some JavaxSwing</rdfs:comment>
	</owl:Class>
	<owl:Class rdf:about="&java-se-6;JavaxSwingTextAPI">
		<rdfs:subClassOf rdf:resource="&j2se-5_0;JavaxSwingTextAPI"/>
		<rdfs:comment xml:lang="en">JavaLibrary implementing the javax.swing.text package for Java SE 6</rdfs:comment>
		<rdfs:comment xml:lang="OWLManchester">platform:comprisesInterfacePart some JavaxSwingText</rdfs:comment>
	</owl:Class>
	<owl:Class rdf:about="&java-se-6;JavaxSwingTextHtmlAPI">
		<rdfs:subClassOf rdf:resource="&j2se-5_0;JavaxSwingTextHtmlAPI"/>
		<rdfs:comment xml:lang="en">JavaLibrary implementing the javax.swing.text.html package for Java SE 6</rdfs:comment>
		<rdfs:comment xml:lang="OWLManchester">platform:comprisesInterfacePart some JavaxSwingTextHtml</rdfs:comment>
	</owl:Class>
	<owl:Class rdf:about="&java-se-6;JavaxSwingTextHtmlParserAPI">
		<owl:equivalentClass rdf:resource="&j2se-5_0;JavaxSwingTextHtmlParserAPI"/>
		<rdfs:subClassOf rdf:resource="&java;JavaAPI"/>
		<rdfs:comment xml:lang="en">JavaLibrary implementing the javax.swing.text.html.parser package for Java SE 6</rdfs:comment>
		<rdfs:comment xml:lang="OWLManchester">platform:comprisesInterfacePart some JavaxSwingTextHtmlParser</rdfs:comment>
	</owl:Class>
	<owl:Class rdf:about="&java-se-6;JavaxSwingTextRtfAPI">
		<rdfs:subClassOf rdf:resource="&j2se-5_0;JavaxSwingTextRtfAPI"/>
		<rdfs:comment xml:lang="en">JavaLibrary implementing the javax.swing.text.rtf package for Java SE 6</rdfs:comment>
		<rdfs:comment xml:lang="OWLManchester">platform:comprisesInterfacePart some JavaxSwingTextRtf</rdfs:comment>
	</owl:Class>
	<owl:Class rdf:about="&java-se-6;JavaxSwingEventAPI">
		<rdfs:subClassOf rdf:resource="&j2se-5_0;JavaxSwingEventAPI"/>
		<rdfs:comment xml:lang="en">JavaLibrary implementing the javax.swing.event package for Java SE 6</rdfs:comment>
		<rdfs:comment xml:lang="OWLManchester">platform:comprisesInterfacePart some JavaxSwingEvent</rdfs:comment>
	</owl:Class>
	<owl:Class rdf:about="&java-se-6;JavaxSwingColorchooserAPI">
		<rdfs:subClassOf rdf:resource="&j2se-5_0;JavaxSwingColorchooserAPI"/>
		<rdfs:comment xml:lang="en">JavaLibrary implementing the javax.swing.colorchooser package for Java SE 6</rdfs:comment>
		<rdfs:comment xml:lang="OWLManchester">platform:comprisesInterfacePart some JavaxSwingColorchooser</rdfs:comment>
	</owl:Class>
	<owl:Class rdf:about="&java-se-6;JavaxSwingPlafAPI">
		<rdfs:subClassOf rdf:resource="&j2se-5_0;JavaxSwingPlafAPI"/>
		<rdfs:comment xml:lang="en">JavaLibrary implementing the javax.swing.plaf package for Java SE 6</rdfs:comment>
		<rdfs:comment xml:lang="OWLManchester">platform:comprisesInterfacePart some JavaxSwingPlaf</rdfs:comment>
	</owl:Class>
	<owl:Class rdf:about="&java-se-6;JavaxSwingPlafBasicAPI">
		<rdfs:subClassOf rdf:resource="&j2se-5_0;JavaxSwingPlafBasicAPI"/>
		<rdfs:comment xml:lang="en">JavaLibrary implementing the javax.swing.plaf.basic package for Java SE 6</rdfs:comment>
		<rdfs:comment xml:lang="OWLManchester">platform:comprisesInterfacePart some JavaxSwingPlafBasic</rdfs:comment>
	</owl:Class>
	<owl:Class rdf:about="&java-se-6;JavaxSwingPlafMetalAPI">
		<rdfs:subClassOf rdf:resource="&j2se-5_0;JavaxSwingPlafMetalAPI"/>
		<rdfs:comment xml:lang="en">JavaLibrary implementing the javax.swing.plaf.metal package for Java SE 6</rdfs:comment>
		<rdfs:comment xml:lang="OWLManchester">platform:comprisesInterfacePart some JavaxSwingPlafMetal</rdfs:comment>
	</owl:Class>
	<owl:Class rdf:about="&java-se-6;JavaxSwingPlafMultiAPI">
		<rdfs:subClassOf rdf:resource="&j2se-5_0;JavaxSwingPlafMultiAPI"/>
		<rdfs:comment xml:lang="en">JavaLibrary implementing the javax.swing.plaf.multi package for Java SE 6</rdfs:comment>
		<rdfs:comment xml:lang="OWLManchester">platform:comprisesInterfacePart some JavaxSwingPlafMulti</rdfs:comment>
	</owl:Class>
	<owl:Class rdf:about="&java-se-6;JavaxSwingPlafSynthAPI">
		<rdfs:subClassOf rdf:resource="&j2se-5_0;JavaxSwingPlafSynthAPI"/>
		<rdfs:comment xml:lang="en">JavaLibrary implementing the javax.swing.plaf.synth package for Java SE 6</rdfs:comment>
		<rdfs:comment xml:lang="OWLManchester">platform:comprisesInterfacePart some JavaxSwingPlafSynth</rdfs:comment>
	</owl:Class>
	<owl:Class rdf:about="&java-se-6;JavaxSwingFilechooserAPI">
		<rdfs:subClassOf rdf:resource="&j2se-5_0;JavaxSwingFilechooserAPI"/>
		<rdfs:comment xml:lang="en">JavaLibrary implementing the javax.swing.filechooser package for Java SE 6</rdfs:comment>
		<rdfs:comment xml:lang="OWLManchester">platform:comprisesInterfacePart some JavaxSwingFilechooser</rdfs:comment>
	</owl:Class>
	<owl:Class rdf:about="&java-se-6;JavaxSwingTreeAPI">
		<rdfs:subClassOf rdf:resource="&j2se-5_0;JavaxSwingTreeAPI"/>
		<rdfs:comment xml:lang="en">JavaLibrary implementing the javax.swing.tree package for Java SE 6</rdfs:comment>
		<rdfs:comment xml:lang="OWLManchester">platform:comprisesInterfacePart some JavaxSwingTree</rdfs:comment>
	</owl:Class>
	<owl:Class rdf:about="&java-se-6;JavaxSwingBorderAPI">
		<rdfs:subClassOf rdf:resource="&j2se-5_0;JavaxSwingBorderAPI"/>
		<rdfs:comment xml:lang="en">JavaLibrary implementing the javax.swing.border package for Java SE 6</rdfs:comment>
		<rdfs:comment xml:lang="OWLManchester">platform:comprisesInterfacePart some JavaxSwingBorder</rdfs:comment>
	</owl:Class>
	<owl:Class rdf:about="&java-se-6;JavaxSwingTableAPI">
		<rdfs:subClassOf rdf:resource="&j2se-5_0;JavaxSwingTableAPI"/>
		<rdfs:comment xml:lang="en">JavaLibrary implementing the javax.swing.table package for Java SE 6</rdfs:comment>
		<rdfs:comment xml:lang="OWLManchester">platform:comprisesInterfacePart some JavaxSwingTable</rdfs:comment>
	</owl:Class>
	<owl:Class rdf:about="&java-se-6;JavaxSwingUndoAPI">
		<owl:equivalentClass rdf:resource="&j2se-5_0;JavaxSwingUndoAPI"/>
		<rdfs:subClassOf rdf:resource="&java;JavaAPI"/>
		<rdfs:comment xml:lang="en">JavaLibrary implementing the javax.swing.undo package for Java SE 6</rdfs:comment>
		<rdfs:comment xml:lang="OWLManchester">platform:comprisesInterfacePart some JavaxSwingUndo</rdfs:comment>
	</owl:Class>
	<owl:Class rdf:about="&java-se-6;JavaxManagementAPI">
		<rdfs:subClassOf rdf:resource="&j2se-5_0;JavaxManagementAPI"/>
		<rdfs:comment xml:lang="en">JavaLibrary implementing the javax.management package for Java SE 6</rdfs:comment>
		<rdfs:comment xml:lang="OWLManchester">platform:comprisesInterfacePart some JavaxManagement</rdfs:comment>
	</owl:Class>
	<owl:Class rdf:about="&java-se-6;JavaxManagementOpenmbeanAPI">
		<rdfs:subClassOf rdf:resource="&j2se-5_0;JavaxManagementOpenmbeanAPI"/>
		<rdfs:comment xml:lang="en">JavaLibrary implementing the javax.management.openmbean package for Java SE 6</rdfs:comment>
		<rdfs:comment xml:lang="OWLManchester">platform:comprisesInterfacePart some JavaxManagementOpenmbean</rdfs:comment>
	</owl:Class>
	<owl:Class rdf:about="&java-se-6;JavaxManagementLoadingAPI">
		<rdfs:subClassOf rdf:resource="&j2se-5_0;JavaxManagementLoadingAPI"/>
		<rdfs:comment xml:lang="en">JavaLibrary implementing the javax.management.loading package for Java SE 6</rdfs:comment>
		<rdfs:comment xml:lang="OWLManchester">platform:comprisesInterfacePart some JavaxManagementLoading</rdfs:comment>
	</owl:Class>
	<owl:Class rdf:about="&java-se-6;JavaxManagementModelmbeanAPI">
		<rdfs:subClassOf rdf:resource="&j2se-5_0;JavaxManagementModelmbeanAPI"/>
		<rdfs:comment xml:lang="en">JavaLibrary implementing the javax.management.modelmbean package for Java SE 6</rdfs:comment>
		<rdfs:comment xml:lang="OWLManchester">platform:comprisesInterfacePart some JavaxManagementModelmbean</rdfs:comment>
	</owl:Class>
	<owl:Class rdf:about="&java-se-6;JavaxManagementMonitorAPI">
		<rdfs:subClassOf rdf:resource="&j2se-5_0;JavaxManagementMonitorAPI"/>
		<rdfs:comment xml:lang="en">JavaLibrary implementing the javax.management.monitor package for Java SE 6</rdfs:comment>
		<rdfs:comment xml:lang="OWLManchester">platform:comprisesInterfacePart some JavaxManagementMonitor</rdfs:comment>
	</owl:Class>
	<owl:Class rdf:about="&java-se-6;JavaxManagementRelationAPI">
		<rdfs:subClassOf rdf:resource="&j2se-5_0;JavaxManagementRelationAPI"/>
		<rdfs:comment xml:lang="en">JavaLibrary implementing the javax.management.relation package for Java SE 6</rdfs:comment>
		<rdfs:comment xml:lang="OWLManchester">platform:comprisesInterfacePart some JavaxManagementRelation</rdfs:comment>
	</owl:Class>
	<owl:Class rdf:about="&java-se-6;JavaxManagementRemoteAPI">
		<rdfs:subClassOf rdf:resource="&j2se-5_0;JavaxManagementRemoteAPI"/>
		<rdfs:comment xml:lang="en">JavaLibrary implementing the javax.management.remote package for Java SE 6</rdfs:comment>
		<rdfs:comment xml:lang="OWLManchester">platform:comprisesInterfacePart some JavaxManagementRemote</rdfs:comment>
	</owl:Class>
	<owl:Class rdf:about="&java-se-6;JavaxManagementRemoteRmiAPI">
		<rdfs:subClassOf rdf:resource="&j2se-5_0;JavaxManagementRemoteRmiAPI"/>
		<rdfs:comment xml:lang="en">JavaLibrary implementing the javax.management.remote.rmi package for Java SE 6</rdfs:comment>
		<rdfs:comment xml:lang="OWLManchester">platform:comprisesInterfacePart some JavaxManagementRemoteRmi</rdfs:comment>
	</owl:Class>
	<owl:Class rdf:about="&java-se-6;JavaxManagementTimerAPI">
		<rdfs:subClassOf rdf:resource="&java;JavaAPI"/>
		<rdfs:comment xml:lang="en">JavaLibrary implementing the javax.management.timer package for Java SE 6</rdfs:comment>
		<rdfs:comment xml:lang="OWLManchester">platform:comprisesInterfacePart some JavaxManagementTimer</rdfs:comment>
	</owl:Class>
	<owl:Class rdf:about="&java-se-6;JavaxXmlAPI">
		<owl:equivalentClass rdf:resource="&j2se-5_0;JavaxXmlAPI"/>
		<rdfs:subClassOf rdf:resource="&java;JavaAPI"/>
		<rdfs:comment xml:lang="en">JavaLibrary implementing the javax.xml package for Java SE 6</rdfs:comment>
		<rdfs:comment xml:lang="OWLManchester">platform:comprisesInterfacePart some JavaxXml</rdfs:comment>
	</owl:Class>
	<owl:Class rdf:about="&java-se-6;JavaxXmlTransformAPI">
		<rdfs:subClassOf rdf:resource="&j2se-5_0;JavaxXmlTransformAPI"/>
		<rdfs:comment xml:lang="en">JavaLibrary implementing the javax.xml.transform package for Java SE 6</rdfs:comment>
		<rdfs:comment xml:lang="OWLManchester">platform:comprisesInterfacePart some JavaxXmlTransform</rdfs:comment>
	</owl:Class>
	<owl:Class rdf:about="&java-se-6;JavaxXmlTransformDomAPI">
		<owl:equivalentClass rdf:resource="&j2se-5_0;JavaxXmlTransformDomAPI"/>
		<rdfs:subClassOf rdf:resource="&java;JavaAPI"/>
		<rdfs:comment xml:lang="en">JavaLibrary implementing the javax.xml.transform.dom package for Java SE 6</rdfs:comment>
		<rdfs:comment xml:lang="OWLManchester">platform:comprisesInterfacePart some JavaxXmlTransformDom</rdfs:comment>
	</owl:Class>
	<owl:Class rdf:about="&java-se-6;JavaxXmlTransformSaxAPI">
		<rdfs:subClassOf rdf:resource="&j2se-5_0;JavaxXmlTransformSaxAPI"/>
		<rdfs:comment xml:lang="en">JavaLibrary implementing the javax.xml.transform.sax package for Java SE 6</rdfs:comment>
		<rdfs:comment xml:lang="OWLManchester">platform:comprisesInterfacePart some JavaxXmlTransformSax</rdfs:comment>
	</owl:Class>
	<owl:Class rdf:about="&java-se-6;JavaxXmlTransformStaxAPI">
		<rdfs:subClassOf rdf:resource="&java;JavaAPI"/>
		<rdfs:comment xml:lang="en">JavaLibrary implementing the javax.xml.transform.stax package for Java SE 6</rdfs:comment>
		<rdfs:comment xml:lang="OWLManchester">platform:comprisesInterfacePart some JavaxXmlTransformStax</rdfs:comment>
	</owl:Class>
	<owl:Class rdf:about="&java-se-6;JavaxXmlTransformStreamAPI">
		<owl:equivalentClass rdf:resource="&j2se-5_0;JavaxXmlTransformStreamAPI"/>
		<rdfs:subClassOf rdf:resource="&java;JavaAPI"/>
		<rdfs:comment xml:lang="en">JavaLibrary implementing the javax.xml.transform.stream package for Java SE 6</rdfs:comment>
		<rdfs:comment xml:lang="OWLManchester">platform:comprisesInterfacePart some JavaxXmlTransformStream</rdfs:comment>
	</owl:Class>
	<owl:Class rdf:about="&java-se-6;JavaxXmlBindAPI">
		<rdfs:subClassOf rdf:resource="&java;JavaAPI"/>
		<rdfs:comment xml:lang="en">JavaLibrary implementing the javax.xml.bind package for Java SE 6</rdfs:comment>
		<rdfs:comment xml:lang="OWLManchester">platform:comprisesInterfacePart some JavaxXmlBind</rdfs:comment>
	</owl:Class>
	<owl:Class rdf:about="&java-se-6;JavaxXmlBindAnnotationAPI">
		<rdfs:subClassOf rdf:resource="&java;JavaAPI"/>
		<rdfs:comment xml:lang="en">JavaLibrary implementing the javax.xml.bind.annotation package for Java SE 6</rdfs:comment>
		<rdfs:comment xml:lang="OWLManchester">platform:comprisesInterfacePart some JavaxXmlBindAnnotation</rdfs:comment>
	</owl:Class>
	<owl:Class rdf:about="&java-se-6;JavaxXmlBindAnnotationAdaptersAPI">
		<rdfs:subClassOf rdf:resource="&java;JavaAPI"/>
		<rdfs:comment xml:lang="en">JavaLibrary implementing the javax.xml.bind.annotation.adapters package for Java SE 6</rdfs:comment>
		<rdfs:comment xml:lang="OWLManchester">platform:comprisesInterfacePart some JavaxXmlBindAnnotationAdapters</rdfs:comment>
	</owl:Class>
	<owl:Class rdf:about="&java-se-6;JavaxXmlBindAttachmentAPI">
		<rdfs:subClassOf rdf:resource="&java;JavaAPI"/>
		<rdfs:comment xml:lang="en">JavaLibrary implementing the javax.xml.bind.attachment package for Java SE 6</rdfs:comment>
		<rdfs:comment xml:lang="OWLManchester">platform:comprisesInterfacePart some JavaxXmlBindAttachment</rdfs:comment>
	</owl:Class>
	<owl:Class rdf:about="&java-se-6;JavaxXmlBindHelpersAPI">
		<rdfs:subClassOf rdf:resource="&java;JavaAPI"/>
		<rdfs:comment xml:lang="en">JavaLibrary implementing the javax.xml.bind.helpers package for Java SE 6</rdfs:comment>
		<rdfs:comment xml:lang="OWLManchester">platform:comprisesInterfacePart some JavaxXmlBindHelpers</rdfs:comment>
	</owl:Class>
	<owl:Class rdf:about="&java-se-6;JavaxXmlBindUtilAPI">
		<rdfs:subClassOf rdf:resource="&java;JavaAPI"/>
		<rdfs:comment xml:lang="en">JavaLibrary implementing the javax.xml.bind.util package for Java SE 6</rdfs:comment>
		<rdfs:comment xml:lang="OWLManchester">platform:comprisesInterfacePart some JavaxXmlBindUtil</rdfs:comment>
	</owl:Class>
	<owl:Class rdf:about="&java-se-6;JavaxXmlValidationAPI">
		<rdfs:subClassOf rdf:resource="&j2se-5_0;JavaxXmlValidationAPI"/>
		<rdfs:comment xml:lang="en">JavaLibrary implementing the javax.xml.validation package for Java SE 6</rdfs:comment>
		<rdfs:comment xml:lang="OWLManchester">platform:comprisesInterfacePart some JavaxXmlValidation</rdfs:comment>
	</owl:Class>
	<owl:Class rdf:about="&java-se-6;JavaxXmlNamespaceAPI">
		<owl:equivalentClass rdf:resource="&j2se-5_0;JavaxXmlNamespaceAPI"/>
		<rdfs:subClassOf rdf:resource="&java;JavaAPI"/>
		<rdfs:comment xml:lang="en">JavaLibrary implementing the javax.xml.namespace package for Java SE 6</rdfs:comment>
		<rdfs:comment xml:lang="OWLManchester">platform:comprisesInterfacePart some JavaxXmlNamespace</rdfs:comment>
	</owl:Class>
	<owl:Class rdf:about="&java-se-6;JavaxXmlStreamAPI">
		<rdfs:subClassOf rdf:resource="&java;JavaAPI"/>
		<rdfs:comment xml:lang="en">JavaLibrary implementing the javax.xml.stream package for Java SE 6</rdfs:comment>
		<rdfs:comment xml:lang="OWLManchester">platform:comprisesInterfacePart some JavaxXmlStream</rdfs:comment>
	</owl:Class>
	<owl:Class rdf:about="&java-se-6;JavaxXmlStreamEventsAPI">
		<rdfs:subClassOf rdf:resource="&java;JavaAPI"/>
		<rdfs:comment xml:lang="en">JavaLibrary implementing the javax.xml.stream.events package for Java SE 6</rdfs:comment>
		<rdfs:comment xml:lang="OWLManchester">platform:comprisesInterfacePart some JavaxXmlStreamEvents</rdfs:comment>
	</owl:Class>
	<owl:Class rdf:about="&java-se-6;JavaxXmlStreamUtilAPI">
		<rdfs:subClassOf rdf:resource="&java;JavaAPI"/>
		<rdfs:comment xml:lang="en">JavaLibrary implementing the javax.xml.stream.util package for Java SE 6</rdfs:comment>
		<rdfs:comment xml:lang="OWLManchester">platform:comprisesInterfacePart some JavaxXmlStreamUtil</rdfs:comment>
	</owl:Class>
	<owl:Class rdf:about="&java-se-6;JavaxXmlParsersAPI">
		<rdfs:subClassOf rdf:resource="&j2se-5_0;JavaxXmlParsersAPI"/>
		<rdfs:comment xml:lang="en">JavaLibrary implementing the javax.xml.parsers package for Java SE 6</rdfs:comment>
		<rdfs:comment xml:lang="OWLManchester">platform:comprisesInterfacePart some JavaxXmlParsers</rdfs:comment>
	</owl:Class>
	<owl:Class rdf:about="&java-se-6;JavaxXmlCryptoAPI">
		<rdfs:subClassOf rdf:resource="&java;JavaAPI"/>
		<rdfs:comment xml:lang="en">JavaLibrary implementing the javax.xml.crypto package for Java SE 6</rdfs:comment>
		<rdfs:comment xml:lang="OWLManchester">platform:comprisesInterfacePart some JavaxXmlCrypto</rdfs:comment>
	</owl:Class>
	<owl:Class rdf:about="&java-se-6;JavaxXmlCryptoDsigAPI">
		<rdfs:subClassOf rdf:resource="&java;JavaAPI"/>
		<rdfs:comment xml:lang="en">JavaLibrary implementing the javax.xml.crypto.dsig package for Java SE 6</rdfs:comment>
		<rdfs:comment xml:lang="OWLManchester">platform:comprisesInterfacePart some JavaxXmlCryptoDsig</rdfs:comment>
	</owl:Class>
	<owl:Class rdf:about="&java-se-6;JavaxXmlCryptoDsigKeyinfoAPI">
		<rdfs:subClassOf rdf:resource="&java;JavaAPI"/>
		<rdfs:comment xml:lang="en">JavaLibrary implementing the javax.xml.crypto.dsig.keyinfo package for Java SE 6</rdfs:comment>
		<rdfs:comment xml:lang="OWLManchester">platform:comprisesInterfacePart some JavaxXmlCryptoDsigKeyinfo</rdfs:comment>
	</owl:Class>
	<owl:Class rdf:about="&java-se-6;JavaxXmlCryptoDsigSpecAPI">
		<rdfs:subClassOf rdf:resource="&java;JavaAPI"/>
		<rdfs:comment xml:lang="en">JavaLibrary implementing the javax.xml.crypto.dsig.spec package for Java SE 6</rdfs:comment>
		<rdfs:comment xml:lang="OWLManchester">platform:comprisesInterfacePart some JavaxXmlCryptoDsigSpec</rdfs:comment>
	</owl:Class>
	<owl:Class rdf:about="&java-se-6;JavaxXmlCryptoDsigDomAPI">
		<rdfs:subClassOf rdf:resource="&java;JavaAPI"/>
		<rdfs:comment xml:lang="en">JavaLibrary implementing the javax.xml.crypto.dsig.dom package for Java SE 6</rdfs:comment>
		<rdfs:comment xml:lang="OWLManchester">platform:comprisesInterfacePart some JavaxXmlCryptoDsigDom</rdfs:comment>
	</owl:Class>
	<owl:Class rdf:about="&java-se-6;JavaxXmlCryptoDomAPI">
		<rdfs:subClassOf rdf:resource="&java;JavaAPI"/>
		<rdfs:comment xml:lang="en">JavaLibrary implementing the javax.xml.crypto.dom package for Java SE 6</rdfs:comment>
		<rdfs:comment xml:lang="OWLManchester">platform:comprisesInterfacePart some JavaxXmlCryptoDom</rdfs:comment>
	</owl:Class>
	<owl:Class rdf:about="&java-se-6;JavaxXmlDatatypeAPI">
		<rdfs:subClassOf rdf:resource="&j2se-5_0;JavaxXmlDatatypeAPI"/>
		<rdfs:comment xml:lang="en">JavaLibrary implementing the javax.xml.datatype package for Java SE 6</rdfs:comment>
		<rdfs:comment xml:lang="OWLManchester">platform:comprisesInterfacePart some JavaxXmlDatatype</rdfs:comment>
	</owl:Class>
	<owl:Class rdf:about="&java-se-6;JavaxXmlSoapAPI">
		<rdfs:subClassOf rdf:resource="&java;JavaAPI"/>
		<rdfs:comment xml:lang="en">JavaLibrary implementing the javax.xml.soap package for Java SE 6</rdfs:comment>
		<rdfs:comment xml:lang="OWLManchester">platform:comprisesInterfacePart some JavaxXmlSoap</rdfs:comment>
	</owl:Class>
	<owl:Class rdf:about="&java-se-6;JavaxXmlWsAPI">
		<rdfs:subClassOf rdf:resource="&java;JavaAPI"/>
		<rdfs:comment xml:lang="en">JavaLibrary implementing the javax.xml.ws package for Java SE 6</rdfs:comment>
		<rdfs:comment xml:lang="OWLManchester">platform:comprisesInterfacePart some JavaxXmlWs</rdfs:comment>
	</owl:Class>
	<owl:Class rdf:about="&java-se-6;JavaxXmlWsHandlerAPI">
		<rdfs:subClassOf rdf:resource="&java;JavaAPI"/>
		<rdfs:comment xml:lang="en">JavaLibrary implementing the javax.xml.ws.handler package for Java SE 6</rdfs:comment>
		<rdfs:comment xml:lang="OWLManchester">platform:comprisesInterfacePart some JavaxXmlWsHandler</rdfs:comment>
	</owl:Class>
	<owl:Class rdf:about="&java-se-6;JavaxXmlWsHandlerSoapAPI">
		<rdfs:subClassOf rdf:resource="&java;JavaAPI"/>
		<rdfs:comment xml:lang="en">JavaLibrary implementing the javax.xml.ws.handler.soap package for Java SE 6</rdfs:comment>
		<rdfs:comment xml:lang="OWLManchester">platform:comprisesInterfacePart some JavaxXmlWsHandlerSoap</rdfs:comment>
	</owl:Class>
	<owl:Class rdf:about="&java-se-6;JavaxXmlWsHttpAPI">
		<rdfs:subClassOf rdf:resource="&java;JavaAPI"/>
		<rdfs:comment xml:lang="en">JavaLibrary implementing the javax.xml.ws.http package for Java SE 6</rdfs:comment>
		<rdfs:comment xml:lang="OWLManchester">platform:comprisesInterfacePart some JavaxXmlWsHttp</rdfs:comment>
	</owl:Class>
	<owl:Class rdf:about="&java-se-6;JavaxXmlWsSoapAPI">
		<rdfs:subClassOf rdf:resource="&java;JavaAPI"/>
		<rdfs:comment xml:lang="en">JavaLibrary implementing the javax.xml.ws.soap package for Java SE 6</rdfs:comment>
		<rdfs:comment xml:lang="OWLManchester">platform:comprisesInterfacePart some JavaxXmlWsSoap</rdfs:comment>
	</owl:Class>
	<owl:Class rdf:about="&java-se-6;JavaxXmlWsSpiAPI">
		<rdfs:subClassOf rdf:resource="&java;JavaAPI"/>
		<rdfs:comment xml:lang="en">JavaLibrary implementing the javax.xml.ws.spi package for Java SE 6</rdfs:comment>
		<rdfs:comment xml:lang="OWLManchester">platform:comprisesInterfacePart some JavaxXmlWsSpi</rdfs:comment>
	</owl:Class>
	<owl:Class rdf:about="&java-se-6;JavaxXmlWsWsaddressingAPI">
		<rdfs:subClassOf rdf:resource="&java;JavaAPI"/>
		<rdfs:comment xml:lang="en">JavaLibrary implementing the javax.xml.ws.wsaddressing package for Java SE 6</rdfs:comment>
		<rdfs:comment xml:lang="OWLManchester">platform:comprisesInterfacePart some JavaxXmlWsWsaddressing</rdfs:comment>
	</owl:Class>
	<owl:Class rdf:about="&java-se-6;JavaxXmlXpathAPI">
		<rdfs:subClassOf rdf:resource="&j2se-5_0;JavaxXmlXpathAPI"/>
		<rdfs:comment xml:lang="en">JavaLibrary implementing the javax.xml.xpath package for Java SE 6</rdfs:comment>
		<rdfs:comment xml:lang="OWLManchester">platform:comprisesInterfacePart some JavaxXmlXpath</rdfs:comment>
	</owl:Class>
	<owl:Class rdf:about="&java-se-6;JavaxActivationAPI">
		<rdfs:subClassOf rdf:resource="&java;JavaAPI"/>
		<rdfs:comment xml:lang="en">JavaLibrary implementing the javax.activation package for Java SE 6</rdfs:comment>
		<rdfs:comment xml:lang="OWLManchester">platform:comprisesInterfacePart some JavaxActivation</rdfs:comment>
	</owl:Class>
	<owl:Class rdf:about="&java-se-6;JavaxActivityAPI">
		<owl:equivalentClass rdf:resource="&j2se-5_0;JavaxActivityAPI"/>
		<rdfs:subClassOf rdf:resource="&java;JavaAPI"/>
		<rdfs:comment xml:lang="en">JavaLibrary implementing the javax.activity package for Java SE 6</rdfs:comment>
		<rdfs:comment xml:lang="OWLManchester">platform:comprisesInterfacePart some JavaxActivity</rdfs:comment>
	</owl:Class>
	<owl:Class rdf:about="&java-se-6;JavaxAnnotationAPI">
		<rdfs:subClassOf rdf:resource="&java;JavaAPI"/>
		<rdfs:comment xml:lang="en">JavaLibrary implementing the javax.annotation package for Java SE 6</rdfs:comment>
		<rdfs:comment xml:lang="OWLManchester">platform:comprisesInterfacePart some JavaxAnnotation</rdfs:comment>
	</owl:Class>
	<owl:Class rdf:about="&java-se-6;JavaxAnnotationProcessingAPI">
		<rdfs:subClassOf rdf:resource="&java;JavaAPI"/>
		<rdfs:comment xml:lang="en">JavaLibrary implementing the javax.annotation.processing package for Java SE 6</rdfs:comment>
		<rdfs:comment xml:lang="OWLManchester">platform:comprisesInterfacePart some JavaxAnnotationProcessing</rdfs:comment>
	</owl:Class>
	<owl:Class rdf:about="&java-se-6;JavaxLangModelAPI">
		<rdfs:subClassOf rdf:resource="&java;JavaAPI"/>
		<rdfs:comment xml:lang="en">JavaLibrary implementing the javax.lang.model package for Java SE 6</rdfs:comment>
		<rdfs:comment xml:lang="OWLManchester">platform:comprisesInterfacePart some JavaxLangModel</rdfs:comment>
	</owl:Class>
	<owl:Class rdf:about="&java-se-6;JavaxLangModelElementAPI">
		<rdfs:subClassOf rdf:resource="&java;JavaAPI"/>
		<rdfs:comment xml:lang="en">JavaLibrary implementing the javax.lang.model.element package for Java SE 6</rdfs:comment>
		<rdfs:comment xml:lang="OWLManchester">platform:comprisesInterfacePart some JavaxLangModelElement</rdfs:comment>
	</owl:Class>
	<owl:Class rdf:about="&java-se-6;JavaxLangModelUtilAPI">
		<rdfs:subClassOf rdf:resource="&java;JavaAPI"/>
		<rdfs:comment xml:lang="en">JavaLibrary implementing the javax.lang.model.util package for Java SE 6</rdfs:comment>
		<rdfs:comment xml:lang="OWLManchester">platform:comprisesInterfacePart some JavaxLangModelUtil</rdfs:comment>
	</owl:Class>
	<owl:Class rdf:about="&java-se-6;JavaxLangModelTypeAPI">
		<rdfs:subClassOf rdf:resource="&java;JavaAPI"/>
		<rdfs:comment xml:lang="en">JavaLibrary implementing the javax.lang.model.type package for Java SE 6</rdfs:comment>
		<rdfs:comment xml:lang="OWLManchester">platform:comprisesInterfacePart some JavaxLangModelType</rdfs:comment>
	</owl:Class>
	<owl:Class rdf:about="&java-se-6;JavaxToolsAPI">
		<rdfs:subClassOf rdf:resource="&java;JavaAPI"/>
		<rdfs:comment xml:lang="en">JavaLibrary implementing the javax.tools package for Java SE 6</rdfs:comment>
		<rdfs:comment xml:lang="OWLManchester">platform:comprisesInterfacePart some JavaxTools</rdfs:comment>
	</owl:Class>
	<owl:Class rdf:about="&java-se-6;JavaxImageioAPI">
		<rdfs:subClassOf rdf:resource="&j2se-5_0;JavaxImageioAPI"/>
		<rdfs:comment xml:lang="en">JavaLibrary implementing the javax.imageio package for Java SE 6</rdfs:comment>
		<rdfs:comment xml:lang="OWLManchester">platform:comprisesInterfacePart some JavaxImageio</rdfs:comment>
	</owl:Class>
	<owl:Class rdf:about="&java-se-6;JavaxImageioMetadataAPI">
		<owl:equivalentClass rdf:resource="&j2se-5_0;JavaxImageioMetadataAPI"/>
		<rdfs:subClassOf rdf:resource="&java;JavaAPI"/>
		<rdfs:comment xml:lang="en">JavaLibrary implementing the javax.imageio.metadata package for Java SE 6</rdfs:comment>
		<rdfs:comment xml:lang="OWLManchester">platform:comprisesInterfacePart some JavaxImageioMetadata</rdfs:comment>
	</owl:Class>
	<owl:Class rdf:about="&java-se-6;JavaxImageioStreamAPI">
		<owl:equivalentClass rdf:resource="&j2se-5_0;JavaxImageioStreamAPI"/>
		<rdfs:subClassOf rdf:resource="&java;JavaAPI"/>
		<rdfs:comment xml:lang="en">JavaLibrary implementing the javax.imageio.stream package for Java SE 6</rdfs:comment>
		<rdfs:comment xml:lang="OWLManchester">platform:comprisesInterfacePart some JavaxImageioStream</rdfs:comment>
	</owl:Class>
	<owl:Class rdf:about="&java-se-6;JavaxImageioSpiAPI">
		<owl:equivalentClass rdf:resource="&j2se-5_0;JavaxImageioSpiAPI"/>
		<rdfs:subClassOf rdf:resource="&java;JavaAPI"/>
		<rdfs:comment xml:lang="en">JavaLibrary implementing the javax.imageio.spi package for Java SE 6</rdfs:comment>
		<rdfs:comment xml:lang="OWLManchester">platform:comprisesInterfacePart some JavaxImageioSpi</rdfs:comment>
	</owl:Class>
	<owl:Class rdf:about="&java-se-6;JavaxImageioEventAPI">
		<owl:equivalentClass rdf:resource="&j2se-5_0;JavaxImageioEventAPI"/>
		<rdfs:subClassOf rdf:resource="&java;JavaAPI"/>
		<rdfs:comment xml:lang="en">JavaLibrary implementing the javax.imageio.event package for Java SE 6</rdfs:comment>
		<rdfs:comment xml:lang="OWLManchester">platform:comprisesInterfacePart some JavaxImageioEvent</rdfs:comment>
	</owl:Class>
	<owl:Class rdf:about="&java-se-6;JavaxImageioPluginsBmpAPI">
		<owl:equivalentClass rdf:resource="&j2se-5_0;JavaxImageioPluginsBmpAPI"/>
		<rdfs:subClassOf rdf:resource="&java;JavaAPI"/>
		<rdfs:comment xml:lang="en">JavaLibrary implementing the javax.imageio.plugins.bmp package for Java SE 6</rdfs:comment>
		<rdfs:comment xml:lang="OWLManchester">platform:comprisesInterfacePart some JavaxImageioPluginsBmp</rdfs:comment>
	</owl:Class>
	<owl:Class rdf:about="&java-se-6;JavaxImageioPluginsJpegAPI">
		<owl:equivalentClass rdf:resource="&j2se-5_0;JavaxImageioPluginsJpegAPI"/>
		<rdfs:subClassOf rdf:resource="&java;JavaAPI"/>
		<rdfs:comment xml:lang="en">JavaLibrary implementing the javax.imageio.plugins.jpeg package for Java SE 6</rdfs:comment>
		<rdfs:comment xml:lang="OWLManchester">platform:comprisesInterfacePart some JavaxImageioPluginsJpeg</rdfs:comment>
	</owl:Class>
	<owl:Class rdf:about="&java-se-6;JavaxJwsAPI">
		<rdfs:subClassOf rdf:resource="&java;JavaAPI"/>
		<rdfs:comment xml:lang="en">JavaLibrary implementing the javax.jws package for Java SE 6</rdfs:comment>
		<rdfs:comment xml:lang="OWLManchester">platform:comprisesInterfacePart some JavaxJws</rdfs:comment>
	</owl:Class>
	<owl:Class rdf:about="&java-se-6;JavaxJwsSoapAPI">
		<rdfs:subClassOf rdf:resource="&java;JavaAPI"/>
		<rdfs:comment xml:lang="en">JavaLibrary implementing the javax.jws.soap package for Java SE 6</rdfs:comment>
		<rdfs:comment xml:lang="OWLManchester">platform:comprisesInterfacePart some JavaxJwsSoap</rdfs:comment>
	</owl:Class>
	<owl:Class rdf:about="&java-se-6;JavaxRmiAPI">
		<owl:equivalentClass rdf:resource="&j2se-5_0;JavaxRmiAPI"/>
		<rdfs:subClassOf rdf:resource="&java;JavaAPI"/>
		<rdfs:comment xml:lang="en">JavaLibrary implementing the javax.rmi package for Java SE 6</rdfs:comment>
		<rdfs:comment xml:lang="OWLManchester">platform:comprisesInterfacePart some JavaxRmi</rdfs:comment>
	</owl:Class>
	<owl:Class rdf:about="&java-se-6;JavaxRmiCORBAAPI">
		<owl:equivalentClass rdf:resource="&j2se-5_0;JavaxRmiCORBAAPI"/>
		<rdfs:subClassOf rdf:resource="&java;JavaAPI"/>
		<rdfs:comment xml:lang="en">JavaLibrary implementing the javax.rmi.CORBA package for Java SE 6</rdfs:comment>
		<rdfs:comment xml:lang="OWLManchester">platform:comprisesInterfacePart some JavaxRmiCORBA</rdfs:comment>
	</owl:Class>
	<owl:Class rdf:about="&java-se-6;JavaxRmiSslAPI">
		<owl:equivalentClass rdf:resource="&j2se-5_0;JavaxRmiSslAPI"/>
		<rdfs:subClassOf rdf:resource="&java;JavaAPI"/>
		<rdfs:comment xml:lang="en">JavaLibrary implementing the javax.rmi.ssl package for Java SE 6</rdfs:comment>
		<rdfs:comment xml:lang="OWLManchester">platform:comprisesInterfacePart some JavaxRmiSsl</rdfs:comment>
	</owl:Class>
	<owl:Class rdf:about="&java-se-6;JavaxNamingAPI">
		<rdfs:subClassOf rdf:resource="&j2se-5_0;JavaxNamingAPI"/>
		<rdfs:comment xml:lang="en">JavaLibrary implementing the javax.naming package for Java SE 6</rdfs:comment>
		<rdfs:comment xml:lang="OWLManchester">platform:comprisesInterfacePart some JavaxNaming</rdfs:comment>
	</owl:Class>
	<owl:Class rdf:about="&java-se-6;JavaxNamingDirectoryAPI">
		<rdfs:subClassOf rdf:resource="&j2se-5_0;JavaxNamingDirectoryAPI"/>
		<rdfs:comment xml:lang="en">JavaLibrary implementing the javax.naming.directory package for Java SE 6</rdfs:comment>
		<rdfs:comment xml:lang="OWLManchester">platform:comprisesInterfacePart some JavaxNamingDirectory</rdfs:comment>
	</owl:Class>
	<owl:Class rdf:about="&java-se-6;JavaxNamingEventAPI">
		<owl:equivalentClass rdf:resource="&j2se-5_0;JavaxNamingEventAPI"/>
		<rdfs:subClassOf rdf:resource="&java;JavaAPI"/>
		<rdfs:comment xml:lang="en">JavaLibrary implementing the javax.naming.event package for Java SE 6</rdfs:comment>
		<rdfs:comment xml:lang="OWLManchester">platform:comprisesInterfacePart some JavaxNamingEvent</rdfs:comment>
	</owl:Class>
	<owl:Class rdf:about="&java-se-6;JavaxNamingLdapAPI">
		<rdfs:subClassOf rdf:resource="&j2se-5_0;JavaxNamingLdapAPI"/>
		<rdfs:comment xml:lang="en">JavaLibrary implementing the javax.naming.ldap package for Java SE 6</rdfs:comment>
		<rdfs:comment xml:lang="OWLManchester">platform:comprisesInterfacePart some JavaxNamingLdap</rdfs:comment>
	</owl:Class>
	<owl:Class rdf:about="&java-se-6;JavaxNamingSpiAPI">
		<owl:equivalentClass rdf:resource="&j2se-5_0;JavaxNamingSpiAPI"/>
		<rdfs:subClassOf rdf:resource="&java;JavaAPI"/>
		<rdfs:comment xml:lang="en">JavaLibrary implementing the javax.naming.spi package for Java SE 6</rdfs:comment>
		<rdfs:comment xml:lang="OWLManchester">platform:comprisesInterfacePart some JavaxNamingSpi</rdfs:comment>
	</owl:Class>
	<owl:Class rdf:about="&java-se-6;JavaxPrintAPI">
		<owl:equivalentClass rdf:resource="&j2se-5_0;JavaxPrintAPI"/>
		<rdfs:subClassOf rdf:resource="&java;JavaAPI"/>
		<rdfs:comment xml:lang="en">JavaLibrary implementing the javax.print package for Java SE 6</rdfs:comment>
		<rdfs:comment xml:lang="OWLManchester">platform:comprisesInterfacePart some JavaxPrint</rdfs:comment>
	</owl:Class>
	<owl:Class rdf:about="&java-se-6;JavaxPrintAttributeAPI">
		<owl:equivalentClass rdf:resource="&j2se-5_0;JavaxPrintAttributeAPI"/>
		<rdfs:subClassOf rdf:resource="&java;JavaAPI"/>
		<rdfs:comment xml:lang="en">JavaLibrary implementing the javax.print.attribute package for Java SE 6</rdfs:comment>
		<rdfs:comment xml:lang="OWLManchester">platform:comprisesInterfacePart some JavaxPrintAttribute</rdfs:comment>
	</owl:Class>
	<owl:Class rdf:about="&java-se-6;JavaxPrintAttributeStandardAPI">
		<owl:equivalentClass rdf:resource="&j2se-5_0;JavaxPrintAttributeStandardAPI"/>
		<rdfs:subClassOf rdf:resource="&java;JavaAPI"/>
		<rdfs:comment xml:lang="en">JavaLibrary implementing the javax.print.attribute.standard package for Java SE 6</rdfs:comment>
		<rdfs:comment xml:lang="OWLManchester">platform:comprisesInterfacePart some JavaxPrintAttributeStandard</rdfs:comment>
	</owl:Class>
	<owl:Class rdf:about="&java-se-6;JavaxPrintEventAPI">
		<owl:equivalentClass rdf:resource="&j2se-5_0;JavaxPrintEventAPI"/>
		<rdfs:subClassOf rdf:resource="&java;JavaAPI"/>
		<rdfs:comment xml:lang="en">JavaLibrary implementing the javax.print.event package for Java SE 6</rdfs:comment>
		<rdfs:comment xml:lang="OWLManchester">platform:comprisesInterfacePart some JavaxPrintEvent</rdfs:comment>
	</owl:Class>
	<owl:Class rdf:about="&java-se-6;JavaxScriptAPI">
		<rdfs:subClassOf rdf:resource="&java;JavaAPI"/>
		<rdfs:comment xml:lang="en">JavaLibrary implementing the javax.script package for Java SE 6</rdfs:comment>
		<rdfs:comment xml:lang="OWLManchester">platform:comprisesInterfacePart some JavaxScript</rdfs:comment>
	</owl:Class>
	<owl:Class rdf:about="&java-se-6;JavaxSmartcardioAPI">
		<rdfs:subClassOf rdf:resource="&java;JavaAPI"/>
		<rdfs:comment xml:lang="en">JavaLibrary implementing the javax.smartcardio package for Java SE 6</rdfs:comment>
		<rdfs:comment xml:lang="OWLManchester">platform:comprisesInterfacePart some JavaxSmartcardio</rdfs:comment>
	</owl:Class>
	<owl:Class rdf:about="&java-se-6;JavaxSoundMidiAPI">
		<owl:equivalentClass rdf:resource="&j2se-5_0;JavaxSoundMidiAPI"/>
		<rdfs:subClassOf rdf:resource="&java;JavaAPI"/>
		<rdfs:comment xml:lang="en">JavaLibrary implementing the javax.sound.midi package for Java SE 6</rdfs:comment>
		<rdfs:comment xml:lang="OWLManchester">platform:comprisesInterfacePart some JavaxSoundMidi</rdfs:comment>
	</owl:Class>
	<owl:Class rdf:about="&java-se-6;JavaxSoundMidiSpiAPI">
		<owl:equivalentClass rdf:resource="&j2se-5_0;JavaxSoundMidiSpiAPI"/>
		<rdfs:subClassOf rdf:resource="&java;JavaAPI"/>
		<rdfs:comment xml:lang="en">JavaLibrary implementing the javax.sound.midi.spi package for Java SE 6</rdfs:comment>
		<rdfs:comment xml:lang="OWLManchester">platform:comprisesInterfacePart some JavaxSoundMidiSpi</rdfs:comment>
	</owl:Class>
	<owl:Class rdf:about="&java-se-6;JavaxSoundSampledAPI">
		<owl:equivalentClass rdf:resource="&j2se-5_0;JavaxSoundSampledAPI"/>
		<rdfs:subClassOf rdf:resource="&java;JavaAPI"/>
		<rdfs:comment xml:lang="en">JavaLibrary implementing the javax.sound.sampled package for Java SE 6</rdfs:comment>
		<rdfs:comment xml:lang="OWLManchester">platform:comprisesInterfacePart some JavaxSoundSampled</rdfs:comment>
	</owl:Class>
	<owl:Class rdf:about="&java-se-6;JavaxSoundSampledSpiAPI">
		<owl:equivalentClass rdf:resource="&j2se-5_0;JavaxSoundSampledSpiAPI"/>
		<rdfs:subClassOf rdf:resource="&java;JavaAPI"/>
		<rdfs:comment xml:lang="en">JavaLibrary implementing the javax.sound.sampled.spi package for Java SE 6</rdfs:comment>
		<rdfs:comment xml:lang="OWLManchester">platform:comprisesInterfacePart some JavaxSoundSampledSpi</rdfs:comment>
	</owl:Class>
	<owl:Class rdf:about="&java-se-6;JavaxSqlAPI">
		<rdfs:subClassOf rdf:resource="&j2se-5_0;JavaxSqlAPI"/>
		<rdfs:comment xml:lang="en">JavaLibrary implementing the javax.sql package for Java SE 6</rdfs:comment>
		<rdfs:comment xml:lang="OWLManchester">platform:comprisesInterfacePart some JavaxSql</rdfs:comment>
	</owl:Class>
	<owl:Class rdf:about="&java-se-6;JavaxSqlRowsetAPI">
		<rdfs:subClassOf rdf:resource="&j2se-5_0;JavaxSqlRowsetAPI"/>
		<rdfs:comment xml:lang="en">JavaLibrary implementing the javax.sql.rowset package for Java SE 6</rdfs:comment>
		<rdfs:comment xml:lang="OWLManchester">platform:comprisesInterfacePart some JavaxSqlRowset</rdfs:comment>
	</owl:Class>
	<owl:Class rdf:about="&java-se-6;JavaxSqlRowsetSpiAPI">
		<rdfs:subClassOf rdf:resource="&j2se-5_0;JavaxSqlRowsetSpiAPI"/>
		<rdfs:comment xml:lang="en">JavaLibrary implementing the javax.sql.rowset.spi package for Java SE 6</rdfs:comment>
		<rdfs:comment xml:lang="OWLManchester">platform:comprisesInterfacePart some JavaxSqlRowsetSpi</rdfs:comment>
	</owl:Class>
	<owl:Class rdf:about="&java-se-6;JavaxSqlRowsetSerialAPI">
		<rdfs:subClassOf rdf:resource="&j2se-5_0;JavaxSqlRowsetSerialAPI"/>
		<rdfs:comment xml:lang="en">JavaLibrary implementing the javax.sql.rowset.serial package for Java SE 6</rdfs:comment>
		<rdfs:comment xml:lang="OWLManchester">platform:comprisesInterfacePart some JavaxSqlRowsetSerial</rdfs:comment>
	</owl:Class>
	<owl:Class rdf:about="&java-se-6;JavaxTransactionAPI">
		<owl:equivalentClass rdf:resource="&j2se-5_0;JavaxTransactionAPI"/>
		<rdfs:subClassOf rdf:resource="&java;JavaAPI"/>
		<rdfs:comment xml:lang="en">JavaLibrary implementing the javax.transaction package for Java SE 6</rdfs:comment>
		<rdfs:comment xml:lang="OWLManchester">platform:comprisesInterfacePart some JavaxTransaction</rdfs:comment>
	</owl:Class>
	<owl:Class rdf:about="&java-se-6;JavaxTransactionXaAPI">
		<owl:equivalentClass rdf:resource="&j2se-5_0;JavaxTransactionXaAPI"/>
		<rdfs:subClassOf rdf:resource="&java;JavaAPI"/>
		<rdfs:comment xml:lang="en">JavaLibrary implementing the javax.transaction.xa package for Java SE 6</rdfs:comment>
		<rdfs:comment xml:lang="OWLManchester">platform:comprisesInterfacePart some JavaxTransactionXa</rdfs:comment>
	</owl:Class>
	<owl:Class rdf:about="&java-se-6;JavaLangAPI">
		<rdfs:subClassOf rdf:resource="&j2se-5_0;JavaLangAPI"/>
		<rdfs:comment xml:lang="en">JavaLibrary implementing the java.lang package for Java SE 6</rdfs:comment>
		<rdfs:comment xml:lang="OWLManchester">platform:comprisesInterfacePart some JavaLang</rdfs:comment>
	</owl:Class>
	<owl:Class rdf:about="&java-se-6;JavaLangAnnotationAPI">
		<rdfs:subClassOf rdf:resource="&j2se-5_0;JavaLangAnnotationAPI"/>
		<rdfs:comment xml:lang="en">JavaLibrary implementing the java.lang.annotation package for Java SE 6</rdfs:comment>
		<rdfs:comment xml:lang="OWLManchester">platform:comprisesInterfacePart some JavaLangAnnotation</rdfs:comment>
	</owl:Class>
	<owl:Class rdf:about="&java-se-6;JavaLangReflectAPI">
		<owl:equivalentClass rdf:resource="&j2se-5_0;JavaLangReflectAPI"/>
		<rdfs:subClassOf rdf:resource="&java;JavaAPI"/>
		<rdfs:comment xml:lang="en">JavaLibrary implementing the java.lang.reflect package for Java SE 6</rdfs:comment>
		<rdfs:comment xml:lang="OWLManchester">platform:comprisesInterfacePart some JavaLangReflect</rdfs:comment>
	</owl:Class>
	<owl:Class rdf:about="&java-se-6;JavaLangInstrumentAPI">
		<rdfs:subClassOf rdf:resource="&j2se-5_0;JavaLangInstrumentAPI"/>
		<rdfs:comment xml:lang="en">JavaLibrary implementing the java.lang.instrument package for Java SE 6</rdfs:comment>
		<rdfs:comment xml:lang="OWLManchester">platform:comprisesInterfacePart some JavaLangInstrument</rdfs:comment>
	</owl:Class>
	<owl:Class rdf:about="&java-se-6;JavaLangManagementAPI">
		<rdfs:subClassOf rdf:resource="&j2se-5_0;JavaLangManagementAPI"/>
		<rdfs:comment xml:lang="en">JavaLibrary implementing the java.lang.management package for Java SE 6</rdfs:comment>
		<rdfs:comment xml:lang="OWLManchester">platform:comprisesInterfacePart some JavaLangManagement</rdfs:comment>
	</owl:Class>
	<owl:Class rdf:about="&java-se-6;JavaLangRefAPI">
		<owl:equivalentClass rdf:resource="&j2se-5_0;JavaLangRefAPI"/>
		<rdfs:subClassOf rdf:resource="&java;JavaAPI"/>
		<rdfs:comment xml:lang="en">JavaLibrary implementing the java.lang.ref package for Java SE 6</rdfs:comment>
		<rdfs:comment xml:lang="OWLManchester">platform:comprisesInterfacePart some JavaLangRef</rdfs:comment>
	</owl:Class>
	<owl:Class rdf:about="&java-se-6;JavaAwtAPI">
		<rdfs:subClassOf rdf:resource="&j2se-5_0;JavaAwtAPI"/>
		<rdfs:comment xml:lang="en">JavaLibrary implementing the java.awt package for Java SE 6</rdfs:comment>
		<rdfs:comment xml:lang="OWLManchester">platform:comprisesInterfacePart some JavaAwt</rdfs:comment>
	</owl:Class>
	<owl:Class rdf:about="&java-se-6;JavaAwtPrintAPI">
		<rdfs:subClassOf rdf:resource="&j2se-5_0;JavaAwtPrintAPI"/>
		<rdfs:comment xml:lang="en">JavaLibrary implementing the java.awt.print package for Java SE 6</rdfs:comment>
		<rdfs:comment xml:lang="OWLManchester">platform:comprisesInterfacePart some JavaAwtPrint</rdfs:comment>
	</owl:Class>
	<owl:Class rdf:about="&java-se-6;JavaAwtDatatransferAPI">
		<owl:equivalentClass rdf:resource="&j2se-5_0;JavaAwtDatatransferAPI"/>
		<rdfs:subClassOf rdf:resource="&java;JavaAPI"/>
		<rdfs:comment xml:lang="en">JavaLibrary implementing the java.awt.datatransfer package for Java SE 6</rdfs:comment>
		<rdfs:comment xml:lang="OWLManchester">platform:comprisesInterfacePart some JavaAwtDatatransfer</rdfs:comment>
	</owl:Class>
	<owl:Class rdf:about="&java-se-6;JavaAwtEventAPI">
		<rdfs:subClassOf rdf:resource="&j2se-5_0;JavaAwtEventAPI"/>
		<rdfs:comment xml:lang="en">JavaLibrary implementing the java.awt.event package for Java SE 6</rdfs:comment>
		<rdfs:comment xml:lang="OWLManchester">platform:comprisesInterfacePart some JavaAwtEvent</rdfs:comment>
	</owl:Class>
	<owl:Class rdf:about="&java-se-6;JavaAwtImageAPI">
		<rdfs:subClassOf rdf:resource="&j2se-5_0;JavaAwtImageAPI"/>
		<rdfs:comment xml:lang="en">JavaLibrary implementing the java.awt.image package for Java SE 6</rdfs:comment>
		<rdfs:comment xml:lang="OWLManchester">platform:comprisesInterfacePart some JavaAwtImage</rdfs:comment>
	</owl:Class>
	<owl:Class rdf:about="&java-se-6;JavaAwtImageRenderableAPI">
		<owl:equivalentClass rdf:resource="&j2se-5_0;JavaAwtImageRenderableAPI"/>
		<rdfs:subClassOf rdf:resource="&java;JavaAPI"/>
		<rdfs:comment xml:lang="en">JavaLibrary implementing the java.awt.image.renderable package for Java SE 6</rdfs:comment>
		<rdfs:comment xml:lang="OWLManchester">platform:comprisesInterfacePart some JavaAwtImageRenderable</rdfs:comment>
	</owl:Class>
	<owl:Class rdf:about="&java-se-6;JavaAwtGeomAPI">
		<rdfs:subClassOf rdf:resource="&java;JavaAPI"/>
		<rdfs:comment xml:lang="en">JavaLibrary implementing the java.awt.geom package for Java SE 6</rdfs:comment>
		<rdfs:comment xml:lang="OWLManchester">platform:comprisesInterfacePart some JavaAwtGeom</rdfs:comment>
	</owl:Class>
	<owl:Class rdf:about="&java-se-6;JavaAwtImAPI">
		<owl:equivalentClass rdf:resource="&j2se-5_0;JavaAwtImAPI"/>
		<rdfs:subClassOf rdf:resource="&java;JavaAPI"/>
		<rdfs:comment xml:lang="en">JavaLibrary implementing the java.awt.im package for Java SE 6</rdfs:comment>
		<rdfs:comment xml:lang="OWLManchester">platform:comprisesInterfacePart some JavaAwtIm</rdfs:comment>
	</owl:Class>
	<owl:Class rdf:about="&java-se-6;JavaAwtImSpiAPI">
		<owl:equivalentClass rdf:resource="&j2se-5_0;JavaAwtImSpiAPI"/>
		<rdfs:subClassOf rdf:resource="&java;JavaAPI"/>
		<rdfs:comment xml:lang="en">JavaLibrary implementing the java.awt.im.spi package for Java SE 6</rdfs:comment>
		<rdfs:comment xml:lang="OWLManchester">platform:comprisesInterfacePart some JavaAwtImSpi</rdfs:comment>
	</owl:Class>
	<owl:Class rdf:about="&java-se-6;JavaAwtColorAPI">
		<owl:equivalentClass rdf:resource="&j2se-5_0;JavaAwtColorAPI"/>
		<rdfs:subClassOf rdf:resource="&java;JavaAPI"/>
		<rdfs:comment xml:lang="en">JavaLibrary implementing the java.awt.color package for Java SE 6</rdfs:comment>
		<rdfs:comment xml:lang="OWLManchester">platform:comprisesInterfacePart some JavaAwtColor</rdfs:comment>
	</owl:Class>
	<owl:Class rdf:about="&java-se-6;JavaAwtDndAPI">
		<owl:equivalentClass rdf:resource="&j2se-5_0;JavaAwtDndAPI"/>
		<rdfs:subClassOf rdf:resource="&java;JavaAPI"/>
		<rdfs:comment xml:lang="en">JavaLibrary implementing the java.awt.dnd package for Java SE 6</rdfs:comment>
		<rdfs:comment xml:lang="OWLManchester">platform:comprisesInterfacePart some JavaAwtDnd</rdfs:comment>
	</owl:Class>
	<owl:Class rdf:about="&java-se-6;JavaAwtFontAPI">
		<rdfs:subClassOf rdf:resource="&j2se-5_0;JavaAwtFontAPI"/>
		<rdfs:comment xml:lang="en">JavaLibrary implementing the java.awt.font package for Java SE 6</rdfs:comment>
		<rdfs:comment xml:lang="OWLManchester">platform:comprisesInterfacePart some JavaAwtFont</rdfs:comment>
	</owl:Class>
	<owl:Class rdf:about="&java-se-6;JavaNetAPI">
		<rdfs:subClassOf rdf:resource="&j2se-5_0;JavaNetAPI"/>
		<rdfs:comment xml:lang="en">JavaLibrary implementing the java.net package for Java SE 6</rdfs:comment>
		<rdfs:comment xml:lang="OWLManchester">platform:comprisesInterfacePart some JavaNet</rdfs:comment>
	</owl:Class>
	<owl:Class rdf:about="&java-se-6;JavaIoAPI">
		<rdfs:subClassOf rdf:resource="&j2se-5_0;JavaIoAPI"/>
		<rdfs:comment xml:lang="en">JavaLibrary implementing the java.io package for Java SE 6</rdfs:comment>
		<rdfs:comment xml:lang="OWLManchester">platform:comprisesInterfacePart some JavaIo</rdfs:comment>
	</owl:Class>
	<owl:Class rdf:about="&java-se-6;JavaSecurityAPI">
		<rdfs:subClassOf rdf:resource="&j2se-5_0;JavaSecurityAPI"/>
		<rdfs:comment xml:lang="en">JavaLibrary implementing the java.security package for Java SE 6</rdfs:comment>
		<rdfs:comment xml:lang="OWLManchester">platform:comprisesInterfacePart some JavaSecurity</rdfs:comment>
	</owl:Class>
	<owl:Class rdf:about="&java-se-6;JavaSecuritySpecAPI">
		<owl:equivalentClass rdf:resource="&j2se-5_0;JavaSecuritySpecAPI"/>
		<rdfs:subClassOf rdf:resource="&java;JavaAPI"/>
		<rdfs:comment xml:lang="en">JavaLibrary implementing the java.security.spec package for Java SE 6</rdfs:comment>
		<rdfs:comment xml:lang="OWLManchester">platform:comprisesInterfacePart some JavaSecuritySpec</rdfs:comment>
	</owl:Class>
	<owl:Class rdf:about="&java-se-6;JavaSecurityCertAPI">
		<owl:equivalentClass rdf:resource="&j2se-5_0;JavaSecurityCertAPI"/>
		<rdfs:subClassOf rdf:resource="&java;JavaAPI"/>
		<rdfs:comment xml:lang="en">JavaLibrary implementing the java.security.cert package for Java SE 6</rdfs:comment>
		<rdfs:comment xml:lang="OWLManchester">platform:comprisesInterfacePart some JavaSecurityCert</rdfs:comment>
	</owl:Class>
	<owl:Class rdf:about="&java-se-6;JavaSecurityAclAPI">
		<owl:equivalentClass rdf:resource="&j2se-5_0;JavaSecurityAclAPI"/>
		<rdfs:subClassOf rdf:resource="&java;JavaAPI"/>
		<rdfs:comment xml:lang="en">JavaLibrary implementing the java.security.acl package for Java SE 6</rdfs:comment>
		<rdfs:comment xml:lang="OWLManchester">platform:comprisesInterfacePart some JavaSecurityAcl</rdfs:comment>
	</owl:Class>
	<owl:Class rdf:about="&java-se-6;JavaSecurityInterfacesAPI">
		<owl:equivalentClass rdf:resource="&j2se-5_0;JavaSecurityInterfacesAPI"/>
		<rdfs:subClassOf rdf:resource="&java;JavaAPI"/>
		<rdfs:comment xml:lang="en">JavaLibrary implementing the java.security.interfaces package for Java SE 6</rdfs:comment>
		<rdfs:comment xml:lang="OWLManchester">platform:comprisesInterfacePart some JavaSecurityInterfaces</rdfs:comment>
	</owl:Class>
	<owl:Class rdf:about="&java-se-6;JavaMathAPI">
		<rdfs:subClassOf rdf:resource="&j2se-5_0;JavaMathAPI"/>
		<rdfs:comment xml:lang="en">JavaLibrary implementing the java.math package for Java SE 6</rdfs:comment>
		<rdfs:comment xml:lang="OWLManchester">platform:comprisesInterfacePart some JavaMath</rdfs:comment>
	</owl:Class>
	<owl:Class rdf:about="&java-se-6;JavaNioAPI">
		<rdfs:subClassOf rdf:resource="&j2se-5_0;JavaNioAPI"/>
		<rdfs:comment xml:lang="en">JavaLibrary implementing the java.nio package for Java SE 6</rdfs:comment>
		<rdfs:comment xml:lang="OWLManchester">platform:comprisesInterfacePart some JavaNio</rdfs:comment>
	</owl:Class>
	<owl:Class rdf:about="&java-se-6;JavaNioChannelsAPI">
		<owl:equivalentClass rdf:resource="&j2se-5_0;JavaNioChannelsAPI"/>
		<rdfs:subClassOf rdf:resource="&java;JavaAPI"/>
		<rdfs:comment xml:lang="en">JavaLibrary implementing the java.nio.channels package for Java SE 6</rdfs:comment>
		<rdfs:comment xml:lang="OWLManchester">platform:comprisesInterfacePart some JavaNioChannels</rdfs:comment>
	</owl:Class>
	<owl:Class rdf:about="&java-se-6;JavaNioChannelsSpiAPI">
		<owl:equivalentClass rdf:resource="&j2se-5_0;JavaNioChannelsSpiAPI"/>
		<rdfs:subClassOf rdf:resource="&java;JavaAPI"/>
		<rdfs:comment xml:lang="en">JavaLibrary implementing the java.nio.channels.spi package for Java SE 6</rdfs:comment>
		<rdfs:comment xml:lang="OWLManchester">platform:comprisesInterfacePart some JavaNioChannelsSpi</rdfs:comment>
	</owl:Class>
	<owl:Class rdf:about="&java-se-6;JavaNioCharsetAPI">
		<owl:equivalentClass rdf:resource="&j2se-5_0;JavaNioCharsetAPI"/>
		<rdfs:subClassOf rdf:resource="&java;JavaAPI"/>
		<rdfs:comment xml:lang="en">JavaLibrary implementing the java.nio.charset package for Java SE 6</rdfs:comment>
		<rdfs:comment xml:lang="OWLManchester">platform:comprisesInterfacePart some JavaNioCharset</rdfs:comment>
	</owl:Class>
	<owl:Class rdf:about="&java-se-6;JavaNioCharsetSpiAPI">
		<owl:equivalentClass rdf:resource="&j2se-5_0;JavaNioCharsetSpiAPI"/>
		<rdfs:subClassOf rdf:resource="&java;JavaAPI"/>
		<rdfs:comment xml:lang="en">JavaLibrary implementing the java.nio.charset.spi package for Java SE 6</rdfs:comment>
		<rdfs:comment xml:lang="OWLManchester">platform:comprisesInterfacePart some JavaNioCharsetSpi</rdfs:comment>
	</owl:Class>
	<owl:Class rdf:about="&java-se-6;JavaUtilAPI">
		<rdfs:subClassOf rdf:resource="&j2se-5_0;JavaUtilAPI"/>
		<rdfs:comment xml:lang="en">JavaLibrary implementing the java.util package for Java SE 6</rdfs:comment>
		<rdfs:comment xml:lang="OWLManchester">platform:comprisesInterfacePart some JavaUtil</rdfs:comment>
	</owl:Class>
	<owl:Class rdf:about="&java-se-6;JavaUtilJarAPI">
		<owl:equivalentClass rdf:resource="&j2se-5_0;JavaUtilJarAPI"/>
		<rdfs:subClassOf rdf:resource="&java;JavaAPI"/>
		<rdfs:comment xml:lang="en">JavaLibrary implementing the java.util.jar package for Java SE 6</rdfs:comment>
		<rdfs:comment xml:lang="OWLManchester">platform:comprisesInterfacePart some JavaUtilJar</rdfs:comment>
	</owl:Class>
	<owl:Class rdf:about="&java-se-6;JavaUtilSpiAPI">
		<rdfs:subClassOf rdf:resource="&java;JavaAPI"/>
		<rdfs:comment xml:lang="en">JavaLibrary implementing the java.util.spi package for Java SE 6</rdfs:comment>
		<rdfs:comment xml:lang="OWLManchester">platform:comprisesInterfacePart some JavaUtilSpi</rdfs:comment>
	</owl:Class>
	<owl:Class rdf:about="&java-se-6;JavaUtilConcurrentAPI">
		<rdfs:subClassOf rdf:resource="&java;JavaAPI"/>
		<rdfs:comment xml:lang="en">JavaLibrary implementing the java.util.concurrent package for Java SE 6</rdfs:comment>
		<rdfs:comment xml:lang="OWLManchester">platform:comprisesInterfacePart some JavaUtilConcurrent</rdfs:comment>
	</owl:Class>
	<owl:Class rdf:about="&java-se-6;JavaUtilConcurrentAtomicAPI">
		<rdfs:subClassOf rdf:resource="&j2se-5_0;JavaUtilConcurrentAtomicAPI"/>
		<rdfs:comment xml:lang="en">JavaLibrary implementing the java.util.concurrent.atomic package for Java SE 6</rdfs:comment>
		<rdfs:comment xml:lang="OWLManchester">platform:comprisesInterfacePart some JavaUtilConcurrentAtomic</rdfs:comment>
	</owl:Class>
	<owl:Class rdf:about="&java-se-6;JavaUtilConcurrentLocksAPI">
		<rdfs:subClassOf rdf:resource="&j2se-5_0;JavaUtilConcurrentLocksAPI"/>
		<rdfs:comment xml:lang="en">JavaLibrary implementing the java.util.concurrent.locks package for Java SE 6</rdfs:comment>
		<rdfs:comment xml:lang="OWLManchester">platform:comprisesInterfacePart some JavaUtilConcurrentLocks</rdfs:comment>
	</owl:Class>
	<owl:Class rdf:about="&java-se-6;JavaUtilZipAPI">
		<rdfs:subClassOf rdf:resource="&j2se-5_0;JavaUtilZipAPI"/>
		<rdfs:comment xml:lang="en">JavaLibrary implementing the java.util.zip package for Java SE 6</rdfs:comment>
		<rdfs:comment xml:lang="OWLManchester">platform:comprisesInterfacePart some JavaUtilZip</rdfs:comment>
	</owl:Class>
	<owl:Class rdf:about="&java-se-6;JavaUtilLoggingAPI">
		<rdfs:subClassOf rdf:resource="&j2se-5_0;JavaUtilLoggingAPI"/>
		<rdfs:comment xml:lang="en">JavaLibrary implementing the java.util.logging package for Java SE 6</rdfs:comment>
		<rdfs:comment xml:lang="OWLManchester">platform:comprisesInterfacePart some JavaUtilLogging</rdfs:comment>
	</owl:Class>
	<owl:Class rdf:about="&java-se-6;JavaUtilPrefsAPI">
		<owl:equivalentClass rdf:resource="&j2se-5_0;JavaUtilPrefsAPI"/>
		<rdfs:subClassOf rdf:resource="&java;JavaAPI"/>
		<rdfs:comment xml:lang="en">JavaLibrary implementing the java.util.prefs package for Java SE 6</rdfs:comment>
		<rdfs:comment xml:lang="OWLManchester">platform:comprisesInterfacePart some JavaUtilPrefs</rdfs:comment>
	</owl:Class>
	<owl:Class rdf:about="&java-se-6;JavaUtilRegexAPI">
		<owl:equivalentClass rdf:resource="&j2se-5_0;JavaUtilRegexAPI"/>
		<rdfs:subClassOf rdf:resource="&java;JavaAPI"/>
		<rdfs:comment xml:lang="en">JavaLibrary implementing the java.util.regex package for Java SE 6</rdfs:comment>
		<rdfs:comment xml:lang="OWLManchester">platform:comprisesInterfacePart some JavaUtilRegex</rdfs:comment>
	</owl:Class>
	<owl:Class rdf:about="&java-se-6;JavaAppletAPI">
		<rdfs:subClassOf rdf:resource="&j2se-5_0;JavaAppletAPI"/>
		<rdfs:comment xml:lang="en">JavaLibrary implementing the java.applet package for Java SE 6</rdfs:comment>
		<rdfs:comment xml:lang="OWLManchester">platform:comprisesInterfacePart some JavaApplet</rdfs:comment>
	</owl:Class>
	<owl:Class rdf:about="&java-se-6;JavaBeansAPI">
		<rdfs:subClassOf rdf:resource="&j2se-5_0;JavaBeansAPI"/>
		<rdfs:comment xml:lang="en">JavaLibrary implementing the java.beans package for Java SE 6</rdfs:comment>
		<rdfs:comment xml:lang="OWLManchester">platform:comprisesInterfacePart some JavaBeans</rdfs:comment>
	</owl:Class>
	<owl:Class rdf:about="&java-se-6;JavaBeansBeancontextAPI">
		<owl:equivalentClass rdf:resource="&j2se-5_0;JavaBeansBeancontextAPI"/>
		<rdfs:subClassOf rdf:resource="&java;JavaAPI"/>
		<rdfs:comment xml:lang="en">JavaLibrary implementing the java.beans.beancontext package for Java SE 6</rdfs:comment>
		<rdfs:comment xml:lang="OWLManchester">platform:comprisesInterfacePart some JavaBeansBeancontext</rdfs:comment>
	</owl:Class>
	<owl:Class rdf:about="&java-se-6;JavaTextAPI">
		<rdfs:subClassOf rdf:resource="&java;JavaAPI"/>
		<rdfs:comment xml:lang="en">JavaLibrary implementing the java.text package for Java SE 6</rdfs:comment>
		<rdfs:comment xml:lang="OWLManchester">platform:comprisesInterfacePart some JavaText</rdfs:comment>
	</owl:Class>
	<owl:Class rdf:about="&java-se-6;JavaTextSpiAPI">
		<rdfs:subClassOf rdf:resource="&java;JavaAPI"/>
		<rdfs:comment xml:lang="en">JavaLibrary implementing the java.text.spi package for Java SE 6</rdfs:comment>
		<rdfs:comment xml:lang="OWLManchester">platform:comprisesInterfacePart some JavaTextSpi</rdfs:comment>
	</owl:Class>
	<owl:Class rdf:about="&java-se-6;JavaRmiAPI">
		<owl:equivalentClass rdf:resource="&j2se-5_0;JavaRmiAPI"/>
		<rdfs:subClassOf rdf:resource="&java;JavaAPI"/>
		<rdfs:comment xml:lang="en">JavaLibrary implementing the java.rmi package for Java SE 6</rdfs:comment>
		<rdfs:comment xml:lang="OWLManchester">platform:comprisesInterfacePart some JavaRmi</rdfs:comment>
	</owl:Class>
	<owl:Class rdf:about="&java-se-6;JavaRmiActivationAPI">
		<owl:equivalentClass rdf:resource="&j2se-5_0;JavaRmiActivationAPI"/>
		<rdfs:subClassOf rdf:resource="&java;JavaAPI"/>
		<rdfs:comment xml:lang="en">JavaLibrary implementing the java.rmi.activation package for Java SE 6</rdfs:comment>
		<rdfs:comment xml:lang="OWLManchester">platform:comprisesInterfacePart some JavaRmiActivation</rdfs:comment>
	</owl:Class>
	<owl:Class rdf:about="&java-se-6;JavaRmiServerAPI">
		<rdfs:subClassOf rdf:resource="&j2se-5_0;JavaRmiServerAPI"/>
		<rdfs:comment xml:lang="en">JavaLibrary implementing the java.rmi.server package for Java SE 6</rdfs:comment>
		<rdfs:comment xml:lang="OWLManchester">platform:comprisesInterfacePart some JavaRmiServer</rdfs:comment>
	</owl:Class>
	<owl:Class rdf:about="&java-se-6;JavaRmiDgcAPI">
		<owl:equivalentClass rdf:resource="&j2se-5_0;JavaRmiDgcAPI"/>
		<rdfs:subClassOf rdf:resource="&java;JavaAPI"/>
		<rdfs:comment xml:lang="en">JavaLibrary implementing the java.rmi.dgc package for Java SE 6</rdfs:comment>
		<rdfs:comment xml:lang="OWLManchester">platform:comprisesInterfacePart some JavaRmiDgc</rdfs:comment>
	</owl:Class>
	<owl:Class rdf:about="&java-se-6;JavaRmiRegistryAPI">
		<owl:equivalentClass rdf:resource="&j2se-5_0;JavaRmiRegistryAPI"/>
		<rdfs:subClassOf rdf:resource="&java;JavaAPI"/>
		<rdfs:comment xml:lang="en">JavaLibrary implementing the java.rmi.registry package for Java SE 6</rdfs:comment>
		<rdfs:comment xml:lang="OWLManchester">platform:comprisesInterfacePart some JavaRmiRegistry</rdfs:comment>
	</owl:Class>
	<owl:Class rdf:about="&java-se-6;JavaSqlAPI">
		<rdfs:subClassOf rdf:resource="&j2se-5_0;JavaSqlAPI"/>
		<rdfs:comment xml:lang="en">JavaLibrary implementing the java.sql package for Java SE 6</rdfs:comment>
		<rdfs:comment xml:lang="OWLManchester">platform:comprisesInterfacePart some JavaSql</rdfs:comment>
	</owl:Class>
	<owl:Class rdf:about="&java-se-6;OrgW3cDomAPI">
		<owl:equivalentClass rdf:resource="&j2se-5_0;OrgW3cDomAPI"/>
		<rdfs:subClassOf rdf:resource="&java;JavaAPI"/>
		<rdfs:comment xml:lang="en">JavaLibrary implementing the org.w3c.dom package for Java SE 6</rdfs:comment>
		<rdfs:comment xml:lang="OWLManchester">platform:comprisesInterfacePart some OrgW3cDom</rdfs:comment>
	</owl:Class>
	<owl:Class rdf:about="&java-se-6;OrgW3cDomLsAPI">
		<owl:equivalentClass rdf:resource="&j2se-5_0;OrgW3cDomLsAPI"/>
		<rdfs:subClassOf rdf:resource="&java;JavaAPI"/>
		<rdfs:comment xml:lang="en">JavaLibrary implementing the org.w3c.dom.ls package for Java SE 6</rdfs:comment>
		<rdfs:comment xml:lang="OWLManchester">platform:comprisesInterfacePart some OrgW3cDomLs</rdfs:comment>
	</owl:Class>
	<owl:Class rdf:about="&java-se-6;OrgW3cDomBootstrapAPI">
		<owl:equivalentClass rdf:resource="&j2se-5_0;OrgW3cDomBootstrapAPI"/>
		<rdfs:subClassOf rdf:resource="&java;JavaAPI"/>
		<rdfs:comment xml:lang="en">JavaLibrary implementing the org.w3c.dom.bootstrap package for Java SE 6</rdfs:comment>
		<rdfs:comment xml:lang="OWLManchester">platform:comprisesInterfacePart some OrgW3cDomBootstrap</rdfs:comment>
	</owl:Class>
	<owl:Class rdf:about="&java-se-6;OrgW3cDomCssAPI">
		<owl:equivalentClass rdf:resource="&j2se-5_0;OrgW3cDomCssAPI"/>
		<rdfs:subClassOf rdf:resource="&java;JavaAPI"/>
		<rdfs:comment xml:lang="en">JavaLibrary implementing the org.w3c.dom.css package for Java SE 6</rdfs:comment>
		<rdfs:comment xml:lang="OWLManchester">platform:comprisesInterfacePart some OrgW3cDomCss</rdfs:comment>
	</owl:Class>
	<owl:Class rdf:about="&java-se-6;OrgW3cDomStylesheetsAPI">
		<owl:equivalentClass rdf:resource="&j2se-5_0;OrgW3cDomStylesheetsAPI"/>
		<rdfs:subClassOf rdf:resource="&java;JavaAPI"/>
		<rdfs:comment xml:lang="en">JavaLibrary implementing the org.w3c.dom.stylesheets package for Java SE 6</rdfs:comment>
		<rdfs:comment xml:lang="OWLManchester">platform:comprisesInterfacePart some OrgW3cDomStylesheets</rdfs:comment>
	</owl:Class>
	<owl:Class rdf:about="&java-se-6;OrgW3cDomViewsAPI">
		<owl:equivalentClass rdf:resource="&j2se-5_0;OrgW3cDomViewsAPI"/>
		<rdfs:subClassOf rdf:resource="&java;JavaAPI"/>
		<rdfs:comment xml:lang="en">JavaLibrary implementing the org.w3c.dom.views package for Java SE 6</rdfs:comment>
		<rdfs:comment xml:lang="OWLManchester">platform:comprisesInterfacePart some OrgW3cDomViews</rdfs:comment>
	</owl:Class>
	<owl:Class rdf:about="&java-se-6;OrgW3cDomEventsAPI">
		<owl:equivalentClass rdf:resource="&j2se-5_0;OrgW3cDomEventsAPI"/>
		<rdfs:subClassOf rdf:resource="&java;JavaAPI"/>
		<rdfs:comment xml:lang="en">JavaLibrary implementing the org.w3c.dom.events package for Java SE 6</rdfs:comment>
		<rdfs:comment xml:lang="OWLManchester">platform:comprisesInterfacePart some OrgW3cDomEvents</rdfs:comment>
	</owl:Class>
	<owl:Class rdf:about="&java-se-6;OrgW3cDomHtmlAPI">
		<owl:equivalentClass rdf:resource="&j2se-5_0;OrgW3cDomHtmlAPI"/>
		<rdfs:subClassOf rdf:resource="&java;JavaAPI"/>
		<rdfs:comment xml:lang="en">JavaLibrary implementing the org.w3c.dom.html package for Java SE 6</rdfs:comment>
		<rdfs:comment xml:lang="OWLManchester">platform:comprisesInterfacePart some OrgW3cDomHtml</rdfs:comment>
	</owl:Class>
	<owl:Class rdf:about="&java-se-6;OrgW3cDomTraversalAPI">
		<owl:equivalentClass rdf:resource="&j2se-5_0;OrgW3cDomTraversalAPI"/>
		<rdfs:subClassOf rdf:resource="&java;JavaAPI"/>
		<rdfs:comment xml:lang="en">JavaLibrary implementing the org.w3c.dom.traversal package for Java SE 6</rdfs:comment>
		<rdfs:comment xml:lang="OWLManchester">platform:comprisesInterfacePart some OrgW3cDomTraversal</rdfs:comment>
	</owl:Class>
	<owl:Class rdf:about="&java-se-6;OrgW3cDomRangesAPI">
		<owl:equivalentClass rdf:resource="&j2se-5_0;OrgW3cDomRangesAPI"/>
		<rdfs:subClassOf rdf:resource="&java;JavaAPI"/>
		<rdfs:comment xml:lang="en">JavaLibrary implementing the org.w3c.dom.ranges package for Java SE 6</rdfs:comment>
		<rdfs:comment xml:lang="OWLManchester">platform:comprisesInterfacePart some OrgW3cDomRanges</rdfs:comment>
	</owl:Class>
	<owl:Class rdf:about="&java-se-6;OrgW3cDomXpathAPI">
		<rdfs:subClassOf rdf:resource="&java;JavaAPI"/>
		<rdfs:comment xml:lang="en">JavaLibrary implementing the org.w3c.dom.xpath package for Java SE 6</rdfs:comment>
		<rdfs:comment xml:lang="OWLManchester">platform:comprisesInterfacePart some OrgW3cDomXpath</rdfs:comment>
	</owl:Class>
	<owl:Class rdf:about="&java-se-6;OrgOmgCORBA_2_3API">
		<owl:equivalentClass rdf:resource="&j2se-5_0;OrgOmgCORBA_2_3API"/>
		<rdfs:subClassOf rdf:resource="&java;JavaAPI"/>
		<rdfs:comment xml:lang="en">JavaLibrary implementing the org.omg.CORBA_2_3 package for Java SE 6</rdfs:comment>
		<rdfs:comment xml:lang="OWLManchester">platform:comprisesInterfacePart some OrgOmgCORBA_2_3</rdfs:comment>
	</owl:Class>
	<owl:Class rdf:about="&java-se-6;OrgOmgCORBA_2_3PortableAPI">
		<owl:equivalentClass rdf:resource="&j2se-5_0;OrgOmgCORBA_2_3PortableAPI"/>
		<rdfs:subClassOf rdf:resource="&java;JavaAPI"/>
		<rdfs:comment xml:lang="en">JavaLibrary implementing the org.omg.CORBA_2_3.portable package for Java SE 6</rdfs:comment>
		<rdfs:comment xml:lang="OWLManchester">platform:comprisesInterfacePart some OrgOmgCORBA_2_3Portable</rdfs:comment>
	</owl:Class>
	<owl:Class rdf:about="&java-se-6;OrgOmgCORBAAPI">
		<owl:equivalentClass rdf:resource="&j2se-5_0;OrgOmgCORBAAPI"/>
		<rdfs:subClassOf rdf:resource="&java;JavaAPI"/>
		<rdfs:comment xml:lang="en">JavaLibrary implementing the org.omg.CORBA package for Java SE 6</rdfs:comment>
		<rdfs:comment xml:lang="OWLManchester">platform:comprisesInterfacePart some OrgOmgCORBA</rdfs:comment>
	</owl:Class>
	<owl:Class rdf:about="&java-se-6;OrgOmgCORBAPortableAPI">
		<owl:equivalentClass rdf:resource="&j2se-5_0;OrgOmgCORBAPortableAPI"/>
		<rdfs:subClassOf rdf:resource="&java;JavaAPI"/>
		<rdfs:comment xml:lang="en">JavaLibrary implementing the org.omg.CORBA.portable package for Java SE 6</rdfs:comment>
		<rdfs:comment xml:lang="OWLManchester">platform:comprisesInterfacePart some OrgOmgCORBAPortable</rdfs:comment>
	</owl:Class>
	<owl:Class rdf:about="&java-se-6;OrgOmgCORBADynAnyPackageAPI">
		<owl:equivalentClass rdf:resource="&j2se-5_0;OrgOmgCORBADynAnyPackageAPI"/>
		<rdfs:subClassOf rdf:resource="&java;JavaAPI"/>
		<rdfs:comment xml:lang="en">JavaLibrary implementing the org.omg.CORBA.DynAnyPackage package for Java SE 6</rdfs:comment>
		<rdfs:comment xml:lang="OWLManchester">platform:comprisesInterfacePart some OrgOmgCORBADynAnyPackage</rdfs:comment>
	</owl:Class>
	<owl:Class rdf:about="&java-se-6;OrgOmgCORBAORBPackageAPI">
		<owl:equivalentClass rdf:resource="&j2se-5_0;OrgOmgCORBAORBPackageAPI"/>
		<rdfs:subClassOf rdf:resource="&java;JavaAPI"/>
		<rdfs:comment xml:lang="en">JavaLibrary implementing the org.omg.CORBA.ORBPackage package for Java SE 6</rdfs:comment>
		<rdfs:comment xml:lang="OWLManchester">platform:comprisesInterfacePart some OrgOmgCORBAORBPackage</rdfs:comment>
	</owl:Class>
	<owl:Class rdf:about="&java-se-6;OrgOmgCORBATypeCodePackageAPI">
		<owl:equivalentClass rdf:resource="&j2se-5_0;OrgOmgCORBATypeCodePackageAPI"/>
		<rdfs:subClassOf rdf:resource="&java;JavaAPI"/>
		<rdfs:comment xml:lang="en">JavaLibrary implementing the org.omg.CORBA.TypeCodePackage package for Java SE 6</rdfs:comment>
		<rdfs:comment xml:lang="OWLManchester">platform:comprisesInterfacePart some OrgOmgCORBATypeCodePackage</rdfs:comment>
	</owl:Class>
	<owl:Class rdf:about="&java-se-6;OrgOmgSendingContextAPI">
		<owl:equivalentClass rdf:resource="&j2se-5_0;OrgOmgSendingContextAPI"/>
		<rdfs:subClassOf rdf:resource="&java;JavaAPI"/>
		<rdfs:comment xml:lang="en">JavaLibrary implementing the org.omg.SendingContext package for Java SE 6</rdfs:comment>
		<rdfs:comment xml:lang="OWLManchester">platform:comprisesInterfacePart some OrgOmgSendingContext</rdfs:comment>
	</owl:Class>
	<owl:Class rdf:about="&java-se-6;OrgOmgCosNamingAPI">
		<owl:equivalentClass rdf:resource="&j2se-5_0;OrgOmgCosNamingAPI"/>
		<rdfs:subClassOf rdf:resource="&java;JavaAPI"/>
		<rdfs:comment xml:lang="en">JavaLibrary implementing the org.omg.CosNaming package for Java SE 6</rdfs:comment>
		<rdfs:comment xml:lang="OWLManchester">platform:comprisesInterfacePart some OrgOmgCosNaming</rdfs:comment>
	</owl:Class>
	<owl:Class rdf:about="&java-se-6;OrgOmgCosNamingNamingContextExtPackageAPI">
		<owl:equivalentClass rdf:resource="&j2se-5_0;OrgOmgCosNamingNamingContextExtPackageAPI"/>
		<rdfs:subClassOf rdf:resource="&java;JavaAPI"/>
		<rdfs:comment xml:lang="en">JavaLibrary implementing the org.omg.CosNaming.NamingContextExtPackage package for Java SE 6</rdfs:comment>
		<rdfs:comment xml:lang="OWLManchester">platform:comprisesInterfacePart some OrgOmgCosNamingNamingContextExtPackage</rdfs:comment>
	</owl:Class>
	<owl:Class rdf:about="&java-se-6;OrgOmgCosNamingNamingContextPackageAPI">
		<owl:equivalentClass rdf:resource="&j2se-5_0;OrgOmgCosNamingNamingContextPackageAPI"/>
		<rdfs:subClassOf rdf:resource="&java;JavaAPI"/>
		<rdfs:comment xml:lang="en">JavaLibrary implementing the org.omg.CosNaming.NamingContextPackage package for Java SE 6</rdfs:comment>
		<rdfs:comment xml:lang="OWLManchester">platform:comprisesInterfacePart some OrgOmgCosNamingNamingContextPackage</rdfs:comment>
	</owl:Class>
	<owl:Class rdf:about="&java-se-6;OrgOmgPortableServerAPI">
		<owl:equivalentClass rdf:resource="&j2se-5_0;OrgOmgPortableServerAPI"/>
		<rdfs:subClassOf rdf:resource="&java;JavaAPI"/>
		<rdfs:comment xml:lang="en">JavaLibrary implementing the org.omg.PortableServer package for Java SE 6</rdfs:comment>
		<rdfs:comment xml:lang="OWLManchester">platform:comprisesInterfacePart some OrgOmgPortableServer</rdfs:comment>
	</owl:Class>
	<owl:Class rdf:about="&java-se-6;OrgOmgPortableServerCurrentPackageAPI">
		<owl:equivalentClass rdf:resource="&j2se-5_0;OrgOmgPortableServerCurrentPackageAPI"/>
		<rdfs:subClassOf rdf:resource="&java;JavaAPI"/>
		<rdfs:comment xml:lang="en">JavaLibrary implementing the org.omg.PortableServer.CurrentPackage package for Java SE 6</rdfs:comment>
		<rdfs:comment xml:lang="OWLManchester">platform:comprisesInterfacePart some OrgOmgPortableServerCurrentPackage</rdfs:comment>
	</owl:Class>
	<owl:Class rdf:about="&java-se-6;OrgOmgPortableServerPOAManagerPackageAPI">
		<owl:equivalentClass rdf:resource="&j2se-5_0;OrgOmgPortableServerPOAManagerPackageAPI"/>
		<rdfs:subClassOf rdf:resource="&java;JavaAPI"/>
		<rdfs:comment xml:lang="en">JavaLibrary implementing the org.omg.PortableServer.POAManagerPackage package for Java SE 6</rdfs:comment>
		<rdfs:comment xml:lang="OWLManchester">platform:comprisesInterfacePart some OrgOmgPortableServerPOAManagerPackage</rdfs:comment>
	</owl:Class>
	<owl:Class rdf:about="&java-se-6;OrgOmgPortableServerPOAPackageAPI">
		<owl:equivalentClass rdf:resource="&j2se-5_0;OrgOmgPortableServerPOAPackageAPI"/>
		<rdfs:subClassOf rdf:resource="&java;JavaAPI"/>
		<rdfs:comment xml:lang="en">JavaLibrary implementing the org.omg.PortableServer.POAPackage package for Java SE 6</rdfs:comment>
		<rdfs:comment xml:lang="OWLManchester">platform:comprisesInterfacePart some OrgOmgPortableServerPOAPackage</rdfs:comment>
	</owl:Class>
	<owl:Class rdf:about="&java-se-6;OrgOmgPortableServerPortableAPI">
		<owl:equivalentClass rdf:resource="&j2se-5_0;OrgOmgPortableServerPortableAPI"/>
		<rdfs:subClassOf rdf:resource="&java;JavaAPI"/>
		<rdfs:comment xml:lang="en">JavaLibrary implementing the org.omg.PortableServer.portable package for Java SE 6</rdfs:comment>
		<rdfs:comment xml:lang="OWLManchester">platform:comprisesInterfacePart some OrgOmgPortableServerPortable</rdfs:comment>
	</owl:Class>
	<owl:Class rdf:about="&java-se-6;OrgOmgPortableServerServantLocatorPackageAPI">
		<owl:equivalentClass rdf:resource="&j2se-5_0;OrgOmgPortableServerServantLocatorPackageAPI"/>
		<rdfs:subClassOf rdf:resource="&java;JavaAPI"/>
		<rdfs:comment xml:lang="en">JavaLibrary implementing the org.omg.PortableServer.ServantLocatorPackage package for Java SE 6</rdfs:comment>
		<rdfs:comment xml:lang="OWLManchester">platform:comprisesInterfacePart some OrgOmgPortableServerServantLocatorPackage</rdfs:comment>
	</owl:Class>
	<owl:Class rdf:about="&java-se-6;OrgOmgDynamicAPI">
		<owl:equivalentClass rdf:resource="&j2se-5_0;OrgOmgDynamicAPI"/>
		<rdfs:subClassOf rdf:resource="&java;JavaAPI"/>
		<rdfs:comment xml:lang="en">JavaLibrary implementing the org.omg.Dynamic package for Java SE 6</rdfs:comment>
		<rdfs:comment xml:lang="OWLManchester">platform:comprisesInterfacePart some OrgOmgDynamic</rdfs:comment>
	</owl:Class>
	<owl:Class rdf:about="&java-se-6;OrgOmgDynamicAnyAPI">
		<owl:equivalentClass rdf:resource="&j2se-5_0;OrgOmgDynamicAnyAPI"/>
		<rdfs:subClassOf rdf:resource="&java;JavaAPI"/>
		<rdfs:comment xml:lang="en">JavaLibrary implementing the org.omg.DynamicAny package for Java SE 6</rdfs:comment>
		<rdfs:comment xml:lang="OWLManchester">platform:comprisesInterfacePart some OrgOmgDynamicAny</rdfs:comment>
	</owl:Class>
	<owl:Class rdf:about="&java-se-6;OrgOmgDynamicAnyDynAnyFactoryPackageAPI">
		<owl:equivalentClass rdf:resource="&j2se-5_0;OrgOmgDynamicAnyDynAnyFactoryPackageAPI"/>
		<rdfs:subClassOf rdf:resource="&java;JavaAPI"/>
		<rdfs:comment xml:lang="en">JavaLibrary implementing the org.omg.DynamicAny.DynAnyFactoryPackage package for Java SE 6</rdfs:comment>
		<rdfs:comment xml:lang="OWLManchester">platform:comprisesInterfacePart some OrgOmgDynamicAnyDynAnyFactoryPackage</rdfs:comment>
	</owl:Class>
	<owl:Class rdf:about="&java-se-6;OrgOmgDynamicAnyDynAnyPackageAPI">
		<owl:equivalentClass rdf:resource="&j2se-5_0;OrgOmgDynamicAnyDynAnyPackageAPI"/>
		<rdfs:subClassOf rdf:resource="&java;JavaAPI"/>
		<rdfs:comment xml:lang="en">JavaLibrary implementing the org.omg.DynamicAny.DynAnyPackage package for Java SE 6</rdfs:comment>
		<rdfs:comment xml:lang="OWLManchester">platform:comprisesInterfacePart some OrgOmgDynamicAnyDynAnyPackage</rdfs:comment>
	</owl:Class>
	<owl:Class rdf:about="&java-se-6;OrgOmgIOPAPI">
		<owl:equivalentClass rdf:resource="&j2se-5_0;OrgOmgIOPAPI"/>
		<rdfs:subClassOf rdf:resource="&java;JavaAPI"/>
		<rdfs:comment xml:lang="en">JavaLibrary implementing the org.omg.IOP package for Java SE 6</rdfs:comment>
		<rdfs:comment xml:lang="OWLManchester">platform:comprisesInterfacePart some OrgOmgIOP</rdfs:comment>
	</owl:Class>
	<owl:Class rdf:about="&java-se-6;OrgOmgIOPCodecFactoryPackageAPI">
		<owl:equivalentClass rdf:resource="&j2se-5_0;OrgOmgIOPCodecFactoryPackageAPI"/>
		<rdfs:subClassOf rdf:resource="&java;JavaAPI"/>
		<rdfs:comment xml:lang="en">JavaLibrary implementing the org.omg.IOP.CodecFactoryPackage package for Java SE 6</rdfs:comment>
		<rdfs:comment xml:lang="OWLManchester">platform:comprisesInterfacePart some OrgOmgIOPCodecFactoryPackage</rdfs:comment>
	</owl:Class>
	<owl:Class rdf:about="&java-se-6;OrgOmgIOPCodecPackageAPI">
		<owl:equivalentClass rdf:resource="&j2se-5_0;OrgOmgIOPCodecPackageAPI"/>
		<rdfs:subClassOf rdf:resource="&java;JavaAPI"/>
		<rdfs:comment xml:lang="en">JavaLibrary implementing the org.omg.IOP.CodecPackage package for Java SE 6</rdfs:comment>
		<rdfs:comment xml:lang="OWLManchester">platform:comprisesInterfacePart some OrgOmgIOPCodecPackage</rdfs:comment>
	</owl:Class>
	<owl:Class rdf:about="&java-se-6;OrgOmgMessagingAPI">
		<owl:equivalentClass rdf:resource="&j2se-5_0;OrgOmgMessagingAPI"/>
		<rdfs:subClassOf rdf:resource="&java;JavaAPI"/>
		<rdfs:comment xml:lang="en">JavaLibrary implementing the org.omg.Messaging package for Java SE 6</rdfs:comment>
		<rdfs:comment xml:lang="OWLManchester">platform:comprisesInterfacePart some OrgOmgMessaging</rdfs:comment>
	</owl:Class>
	<owl:Class rdf:about="&java-se-6;OrgOmgPortableInterceptorAPI">
		<owl:equivalentClass rdf:resource="&j2se-5_0;OrgOmgPortableInterceptorAPI"/>
		<rdfs:subClassOf rdf:resource="&java;JavaAPI"/>
		<rdfs:comment xml:lang="en">JavaLibrary implementing the org.omg.PortableInterceptor package for Java SE 6</rdfs:comment>
		<rdfs:comment xml:lang="OWLManchester">platform:comprisesInterfacePart some OrgOmgPortableInterceptor</rdfs:comment>
	</owl:Class>
	<owl:Class rdf:about="&java-se-6;OrgOmgPortableInterceptorORBInitInfoPackageAPI">
		<owl:equivalentClass rdf:resource="&j2se-5_0;OrgOmgPortableInterceptorORBInitInfoPackageAPI"/>
		<rdfs:subClassOf rdf:resource="&java;JavaAPI"/>
		<rdfs:comment xml:lang="en">JavaLibrary implementing the org.omg.PortableInterceptor.ORBInitInfoPackage package for Java SE 6</rdfs:comment>
		<rdfs:comment xml:lang="OWLManchester">platform:comprisesInterfacePart some OrgOmgPortableInterceptorORBInitInfoPackage</rdfs:comment>
	</owl:Class>
	<owl:Class rdf:about="&java-se-6;OrgOmgStubJavaRmiAPI">
		<owl:equivalentClass rdf:resource="&j2se-5_0;OrgOmgStubJavaRmiAPI"/>
		<rdfs:subClassOf rdf:resource="&java;JavaAPI"/>
		<rdfs:comment xml:lang="en">JavaLibrary implementing the org.omg.stub.java.rmi package for Java SE 6</rdfs:comment>
		<rdfs:comment xml:lang="OWLManchester">platform:comprisesInterfacePart some OrgOmgStubJavaRmi</rdfs:comment>
	</owl:Class>
	<owl:Class rdf:about="&java-se-6;OrgOmgStubJavaxManagementRemoteRmiAPI">
		<owl:equivalentClass rdf:resource="&j2se-5_0;OrgOmgStubJavaxManagementRemoteRmiAPI"/>
		<rdfs:subClassOf rdf:resource="&java;JavaAPI"/>
		<rdfs:comment xml:lang="en">JavaLibrary implementing the org.omg.stub.javax.management.remote.rmi package for Java SE 6</rdfs:comment>
		<rdfs:comment xml:lang="OWLManchester">platform:comprisesInterfacePart some OrgOmgStubJavaxManagementRemoteRmi</rdfs:comment>
	</owl:Class>
	<owl:Class rdf:about="&java-se-6;OrgXmlSaxAPI">
		<owl:equivalentClass rdf:resource="&j2se-5_0;OrgXmlSaxAPI"/>
		<rdfs:subClassOf rdf:resource="&java;JavaAPI"/>
		<rdfs:comment xml:lang="en">JavaLibrary implementing the org.xml.sax package for Java SE 6</rdfs:comment>
		<rdfs:comment xml:lang="OWLManchester">platform:comprisesInterfacePart some OrgXmlSax</rdfs:comment>
	</owl:Class>
	<owl:Class rdf:about="&java-se-6;OrgXmlSaxHelpersAPI">
		<owl:equivalentClass rdf:resource="&j2se-5_0;OrgXmlSaxHelpersAPI"/>
		<rdfs:subClassOf rdf:resource="&java;JavaAPI"/>
		<rdfs:comment xml:lang="en">JavaLibrary implementing the org.xml.sax.helpers package for Java SE 6</rdfs:comment>
		<rdfs:comment xml:lang="OWLManchester">platform:comprisesInterfacePart some OrgXmlSaxHelpers</rdfs:comment>
	</owl:Class>
	<owl:Class rdf:about="&java-se-6;OrgXmlSaxExtAPI">
		<owl:equivalentClass rdf:resource="&j2se-5_0;OrgXmlSaxExtAPI"/>
		<rdfs:subClassOf rdf:resource="&java;JavaAPI"/>
		<rdfs:comment xml:lang="en">JavaLibrary implementing the org.xml.sax.ext package for Java SE 6</rdfs:comment>
		<rdfs:comment xml:lang="OWLManchester">platform:comprisesInterfacePart some OrgXmlSaxExt</rdfs:comment>
	</owl:Class>
	<owl:Class rdf:about="&java-se-6;OrgIetfJgssAPI">
		<owl:equivalentClass rdf:resource="&j2se-5_0;OrgIetfJgssAPI"/>
		<rdfs:subClassOf rdf:resource="&java;JavaAPI"/>
		<rdfs:comment xml:lang="en">JavaLibrary implementing the org.ietf.jgss package for Java SE 6</rdfs:comment>
		<rdfs:comment xml:lang="OWLManchester">platform:comprisesInterfacePart some OrgIetfJgss</rdfs:comment>
	</owl:Class>
	<java-se-6:JavaxJnlp rdf:about="&java-se-6;theJavaxJnlpPart">
	</java-se-6:JavaxJnlp>
	<java-se-6:JavaxCrypto rdf:about="&java-se-6;theJavaxCryptoPart">
	</java-se-6:JavaxCrypto>
	<java-se-6:JavaxCryptoInterfaces rdf:about="&java-se-6;theJavaxCryptoInterfacesPart">
	</java-se-6:JavaxCryptoInterfaces>
	<java-se-6:JavaxCryptoSpec rdf:about="&java-se-6;theJavaxCryptoSpecPart">
	</java-se-6:JavaxCryptoSpec>
	<java-se-6:JavaxNet rdf:about="&java-se-6;theJavaxNetPart">
	</java-se-6:JavaxNet>
	<java-se-6:JavaxNetSsl rdf:about="&java-se-6;theJavaxNetSslPart">
	</java-se-6:JavaxNetSsl>
	<java-se-6:JavaxSecurityCert rdf:about="&java-se-6;theJavaxSecurityCertPart">
	</java-se-6:JavaxSecurityCert>
	<java-se-6:JavaxSecurityAuth rdf:about="&java-se-6;theJavaxSecurityAuthPart">
	</java-se-6:JavaxSecurityAuth>
	<java-se-6:JavaxSecurityAuthCallback rdf:about="&java-se-6;theJavaxSecurityAuthCallbackPart">
	</java-se-6:JavaxSecurityAuthCallback>
	<java-se-6:JavaxSecurityAuthLogin rdf:about="&java-se-6;theJavaxSecurityAuthLoginPart">
	</java-se-6:JavaxSecurityAuthLogin>
	<java-se-6:JavaxSecurityAuthX500 rdf:about="&java-se-6;theJavaxSecurityAuthX500Part">
	</java-se-6:JavaxSecurityAuthX500>
	<java-se-6:JavaxSecurityAuthKerberos rdf:about="&java-se-6;theJavaxSecurityAuthKerberosPart">
	</java-se-6:JavaxSecurityAuthKerberos>
	<java-se-6:JavaxSecurityAuthSpi rdf:about="&java-se-6;theJavaxSecurityAuthSpiPart">
	</java-se-6:JavaxSecurityAuthSpi>
	<java-se-6:JavaxSecuritySasl rdf:about="&java-se-6;theJavaxSecuritySaslPart">
	</java-se-6:JavaxSecuritySasl>
	<java-se-6:JavaxAccessibility rdf:about="&java-se-6;theJavaxAccessibilityPart">
	</java-se-6:JavaxAccessibility>
	<java-se-6:JavaxSwing rdf:about="&java-se-6;theJavaxSwingPart">
	</java-se-6:JavaxSwing>
	<java-se-6:JavaxSwingText rdf:about="&java-se-6;theJavaxSwingTextPart">
	</java-se-6:JavaxSwingText>
	<java-se-6:JavaxSwingTextHtml rdf:about="&java-se-6;theJavaxSwingTextHtmlPart">
	</java-se-6:JavaxSwingTextHtml>
	<java-se-6:JavaxSwingTextHtmlParser rdf:about="&java-se-6;theJavaxSwingTextHtmlParserPart">
	</java-se-6:JavaxSwingTextHtmlParser>
	<java-se-6:JavaxSwingTextRtf rdf:about="&java-se-6;theJavaxSwingTextRtfPart">
	</java-se-6:JavaxSwingTextRtf>
	<java-se-6:JavaxSwingEvent rdf:about="&java-se-6;theJavaxSwingEventPart">
	</java-se-6:JavaxSwingEvent>
	<java-se-6:JavaxSwingColorchooser rdf:about="&java-se-6;theJavaxSwingColorchooserPart">
	</java-se-6:JavaxSwingColorchooser>
	<java-se-6:JavaxSwingPlaf rdf:about="&java-se-6;theJavaxSwingPlafPart">
	</java-se-6:JavaxSwingPlaf>
	<java-se-6:JavaxSwingPlafBasic rdf:about="&java-se-6;theJavaxSwingPlafBasicPart">
	</java-se-6:JavaxSwingPlafBasic>
	<java-se-6:JavaxSwingPlafMetal rdf:about="&java-se-6;theJavaxSwingPlafMetalPart">
	</java-se-6:JavaxSwingPlafMetal>
	<java-se-6:JavaxSwingPlafMulti rdf:about="&java-se-6;theJavaxSwingPlafMultiPart">
	</java-se-6:JavaxSwingPlafMulti>
	<java-se-6:JavaxSwingPlafSynth rdf:about="&java-se-6;theJavaxSwingPlafSynthPart">
	</java-se-6:JavaxSwingPlafSynth>
	<java-se-6:JavaxSwingFilechooser rdf:about="&java-se-6;theJavaxSwingFilechooserPart">
	</java-se-6:JavaxSwingFilechooser>
	<java-se-6:JavaxSwingTree rdf:about="&java-se-6;theJavaxSwingTreePart">
	</java-se-6:JavaxSwingTree>
	<java-se-6:JavaxSwingBorder rdf:about="&java-se-6;theJavaxSwingBorderPart">
	</java-se-6:JavaxSwingBorder>
	<java-se-6:JavaxSwingTable rdf:about="&java-se-6;theJavaxSwingTablePart">
	</java-se-6:JavaxSwingTable>
	<java-se-6:JavaxSwingUndo rdf:about="&java-se-6;theJavaxSwingUndoPart">
	</java-se-6:JavaxSwingUndo>
	<java-se-6:JavaxManagement rdf:about="&java-se-6;theJavaxManagementPart">
	</java-se-6:JavaxManagement>
	<java-se-6:JavaxManagementOpenmbean rdf:about="&java-se-6;theJavaxManagementOpenmbeanPart">
	</java-se-6:JavaxManagementOpenmbean>
	<java-se-6:JavaxManagementLoading rdf:about="&java-se-6;theJavaxManagementLoadingPart">
	</java-se-6:JavaxManagementLoading>
	<java-se-6:JavaxManagementModelmbean rdf:about="&java-se-6;theJavaxManagementModelmbeanPart">
	</java-se-6:JavaxManagementModelmbean>
	<java-se-6:JavaxManagementMonitor rdf:about="&java-se-6;theJavaxManagementMonitorPart">
	</java-se-6:JavaxManagementMonitor>
	<java-se-6:JavaxManagementRelation rdf:about="&java-se-6;theJavaxManagementRelationPart">
	</java-se-6:JavaxManagementRelation>
	<java-se-6:JavaxManagementRemote rdf:about="&java-se-6;theJavaxManagementRemotePart">
	</java-se-6:JavaxManagementRemote>
	<java-se-6:JavaxManagementRemoteRmi rdf:about="&java-se-6;theJavaxManagementRemoteRmiPart">
	</java-se-6:JavaxManagementRemoteRmi>
	<java-se-6:JavaxManagementTimer rdf:about="&java-se-6;theJavaxManagementTimerPart">
	</java-se-6:JavaxManagementTimer>
	<java-se-6:JavaxXml rdf:about="&java-se-6;theJavaxXmlPart">
	</java-se-6:JavaxXml>
	<java-se-6:JavaxXmlTransform rdf:about="&java-se-6;theJavaxXmlTransformPart">
	</java-se-6:JavaxXmlTransform>
	<java-se-6:JavaxXmlTransformDom rdf:about="&java-se-6;theJavaxXmlTransformDomPart">
	</java-se-6:JavaxXmlTransformDom>
	<java-se-6:JavaxXmlTransformSax rdf:about="&java-se-6;theJavaxXmlTransformSaxPart">
	</java-se-6:JavaxXmlTransformSax>
	<java-se-6:JavaxXmlTransformStax rdf:about="&java-se-6;theJavaxXmlTransformStaxPart">
	</java-se-6:JavaxXmlTransformStax>
	<java-se-6:JavaxXmlTransformStream rdf:about="&java-se-6;theJavaxXmlTransformStreamPart">
	</java-se-6:JavaxXmlTransformStream>
	<java-se-6:JavaxXmlBind rdf:about="&java-se-6;theJavaxXmlBindPart">
	</java-se-6:JavaxXmlBind>
	<java-se-6:JavaxXmlBindAnnotation rdf:about="&java-se-6;theJavaxXmlBindAnnotationPart">
	</java-se-6:JavaxXmlBindAnnotation>
	<java-se-6:JavaxXmlBindAnnotationAdapters rdf:about="&java-se-6;theJavaxXmlBindAnnotationAdaptersPart">
	</java-se-6:JavaxXmlBindAnnotationAdapters>
	<java-se-6:JavaxXmlBindAttachment rdf:about="&java-se-6;theJavaxXmlBindAttachmentPart">
	</java-se-6:JavaxXmlBindAttachment>
	<java-se-6:JavaxXmlBindHelpers rdf:about="&java-se-6;theJavaxXmlBindHelpersPart">
	</java-se-6:JavaxXmlBindHelpers>
	<java-se-6:JavaxXmlBindUtil rdf:about="&java-se-6;theJavaxXmlBindUtilPart">
	</java-se-6:JavaxXmlBindUtil>
	<java-se-6:JavaxXmlValidation rdf:about="&java-se-6;theJavaxXmlValidationPart">
	</java-se-6:JavaxXmlValidation>
	<java-se-6:JavaxXmlNamespace rdf:about="&java-se-6;theJavaxXmlNamespacePart">
	</java-se-6:JavaxXmlNamespace>
	<java-se-6:JavaxXmlStream rdf:about="&java-se-6;theJavaxXmlStreamPart">
	</java-se-6:JavaxXmlStream>
	<java-se-6:JavaxXmlStreamEvents rdf:about="&java-se-6;theJavaxXmlStreamEventsPart">
	</java-se-6:JavaxXmlStreamEvents>
	<java-se-6:JavaxXmlStreamUtil rdf:about="&java-se-6;theJavaxXmlStreamUtilPart">
	</java-se-6:JavaxXmlStreamUtil>
	<java-se-6:JavaxXmlParsers rdf:about="&java-se-6;theJavaxXmlParsersPart">
	</java-se-6:JavaxXmlParsers>
	<java-se-6:JavaxXmlCrypto rdf:about="&java-se-6;theJavaxXmlCryptoPart">
	</java-se-6:JavaxXmlCrypto>
	<java-se-6:JavaxXmlCryptoDsig rdf:about="&java-se-6;theJavaxXmlCryptoDsigPart">
	</java-se-6:JavaxXmlCryptoDsig>
	<java-se-6:JavaxXmlCryptoDsigKeyinfo rdf:about="&java-se-6;theJavaxXmlCryptoDsigKeyinfoPart">
	</java-se-6:JavaxXmlCryptoDsigKeyinfo>
	<java-se-6:JavaxXmlCryptoDsigSpec rdf:about="&java-se-6;theJavaxXmlCryptoDsigSpecPart">
	</java-se-6:JavaxXmlCryptoDsigSpec>
	<java-se-6:JavaxXmlCryptoDsigDom rdf:about="&java-se-6;theJavaxXmlCryptoDsigDomPart">
	</java-se-6:JavaxXmlCryptoDsigDom>
	<java-se-6:JavaxXmlCryptoDom rdf:about="&java-se-6;theJavaxXmlCryptoDomPart">
	</java-se-6:JavaxXmlCryptoDom>
	<java-se-6:JavaxXmlDatatype rdf:about="&java-se-6;theJavaxXmlDatatypePart">
	</java-se-6:JavaxXmlDatatype>
	<java-se-6:JavaxXmlSoap rdf:about="&java-se-6;theJavaxXmlSoapPart">
	</java-se-6:JavaxXmlSoap>
	<java-se-6:JavaxXmlWs rdf:about="&java-se-6;theJavaxXmlWsPart">
	</java-se-6:JavaxXmlWs>
	<java-se-6:JavaxXmlWsHandler rdf:about="&java-se-6;theJavaxXmlWsHandlerPart">
	</java-se-6:JavaxXmlWsHandler>
	<java-se-6:JavaxXmlWsHandlerSoap rdf:about="&java-se-6;theJavaxXmlWsHandlerSoapPart">
	</java-se-6:JavaxXmlWsHandlerSoap>
	<java-se-6:JavaxXmlWsHttp rdf:about="&java-se-6;theJavaxXmlWsHttpPart">
	</java-se-6:JavaxXmlWsHttp>
	<java-se-6:JavaxXmlWsSoap rdf:about="&java-se-6;theJavaxXmlWsSoapPart">
	</java-se-6:JavaxXmlWsSoap>
	<java-se-6:JavaxXmlWsSpi rdf:about="&java-se-6;theJavaxXmlWsSpiPart">
	</java-se-6:JavaxXmlWsSpi>
	<java-se-6:JavaxXmlWsWsaddressing rdf:about="&java-se-6;theJavaxXmlWsWsaddressingPart">
	</java-se-6:JavaxXmlWsWsaddressing>
	<java-se-6:JavaxXmlXpath rdf:about="&java-se-6;theJavaxXmlXpathPart">
	</java-se-6:JavaxXmlXpath>
	<java-se-6:JavaxActivation rdf:about="&java-se-6;theJavaxActivationPart">
	</java-se-6:JavaxActivation>
	<java-se-6:JavaxActivity rdf:about="&java-se-6;theJavaxActivityPart">
	</java-se-6:JavaxActivity>
	<java-se-6:JavaxAnnotation rdf:about="&java-se-6;theJavaxAnnotationPart">
	</java-se-6:JavaxAnnotation>
	<java-se-6:JavaxAnnotationProcessing rdf:about="&java-se-6;theJavaxAnnotationProcessingPart">
	</java-se-6:JavaxAnnotationProcessing>
	<java-se-6:JavaxLangModel rdf:about="&java-se-6;theJavaxLangModelPart">
	</java-se-6:JavaxLangModel>
	<java-se-6:JavaxLangModelElement rdf:about="&java-se-6;theJavaxLangModelElementPart">
	</java-se-6:JavaxLangModelElement>
	<java-se-6:JavaxLangModelUtil rdf:about="&java-se-6;theJavaxLangModelUtilPart">
	</java-se-6:JavaxLangModelUtil>
	<java-se-6:JavaxLangModelType rdf:about="&java-se-6;theJavaxLangModelTypePart">
	</java-se-6:JavaxLangModelType>
	<java-se-6:JavaxTools rdf:about="&java-se-6;theJavaxToolsPart">
	</java-se-6:JavaxTools>
	<java-se-6:JavaxImageio rdf:about="&java-se-6;theJavaxImageioPart">
	</java-se-6:JavaxImageio>
	<java-se-6:JavaxImageioMetadata rdf:about="&java-se-6;theJavaxImageioMetadataPart">
	</java-se-6:JavaxImageioMetadata>
	<java-se-6:JavaxImageioStream rdf:about="&java-se-6;theJavaxImageioStreamPart">
	</java-se-6:JavaxImageioStream>
	<java-se-6:JavaxImageioSpi rdf:about="&java-se-6;theJavaxImageioSpiPart">
	</java-se-6:JavaxImageioSpi>
	<java-se-6:JavaxImageioEvent rdf:about="&java-se-6;theJavaxImageioEventPart">
	</java-se-6:JavaxImageioEvent>
	<java-se-6:JavaxImageioPluginsBmp rdf:about="&java-se-6;theJavaxImageioPluginsBmpPart">
	</java-se-6:JavaxImageioPluginsBmp>
	<java-se-6:JavaxImageioPluginsJpeg rdf:about="&java-se-6;theJavaxImageioPluginsJpegPart">
	</java-se-6:JavaxImageioPluginsJpeg>
	<java-se-6:JavaxJws rdf:about="&java-se-6;theJavaxJwsPart">
	</java-se-6:JavaxJws>
	<java-se-6:JavaxJwsSoap rdf:about="&java-se-6;theJavaxJwsSoapPart">
	</java-se-6:JavaxJwsSoap>
	<java-se-6:JavaxRmi rdf:about="&java-se-6;theJavaxRmiPart">
	</java-se-6:JavaxRmi>
	<java-se-6:JavaxRmiCORBA rdf:about="&java-se-6;theJavaxRmiCORBAPart">
	</java-se-6:JavaxRmiCORBA>
	<java-se-6:JavaxRmiSsl rdf:about="&java-se-6;theJavaxRmiSslPart">
	</java-se-6:JavaxRmiSsl>
	<java-se-6:JavaxNaming rdf:about="&java-se-6;theJavaxNamingPart">
	</java-se-6:JavaxNaming>
	<java-se-6:JavaxNamingDirectory rdf:about="&java-se-6;theJavaxNamingDirectoryPart">
	</java-se-6:JavaxNamingDirectory>
	<java-se-6:JavaxNamingEvent rdf:about="&java-se-6;theJavaxNamingEventPart">
	</java-se-6:JavaxNamingEvent>
	<java-se-6:JavaxNamingLdap rdf:about="&java-se-6;theJavaxNamingLdapPart">
	</java-se-6:JavaxNamingLdap>
	<java-se-6:JavaxNamingSpi rdf:about="&java-se-6;theJavaxNamingSpiPart">
	</java-se-6:JavaxNamingSpi>
	<java-se-6:JavaxPrint rdf:about="&java-se-6;theJavaxPrintPart">
	</java-se-6:JavaxPrint>
	<java-se-6:JavaxPrintAttribute rdf:about="&java-se-6;theJavaxPrintAttributePart">
	</java-se-6:JavaxPrintAttribute>
	<java-se-6:JavaxPrintAttributeStandard rdf:about="&java-se-6;theJavaxPrintAttributeStandardPart">
	</java-se-6:JavaxPrintAttributeStandard>
	<java-se-6:JavaxPrintEvent rdf:about="&java-se-6;theJavaxPrintEventPart">
	</java-se-6:JavaxPrintEvent>
	<java-se-6:JavaxScript rdf:about="&java-se-6;theJavaxScriptPart">
	</java-se-6:JavaxScript>
	<java-se-6:JavaxSmartcardio rdf:about="&java-se-6;theJavaxSmartcardioPart">
	</java-se-6:JavaxSmartcardio>
	<java-se-6:JavaxSoundMidi rdf:about="&java-se-6;theJavaxSoundMidiPart">
	</java-se-6:JavaxSoundMidi>
	<java-se-6:JavaxSoundMidiSpi rdf:about="&java-se-6;theJavaxSoundMidiSpiPart">
	</java-se-6:JavaxSoundMidiSpi>
	<java-se-6:JavaxSoundSampled rdf:about="&java-se-6;theJavaxSoundSampledPart">
	</java-se-6:JavaxSoundSampled>
	<java-se-6:JavaxSoundSampledSpi rdf:about="&java-se-6;theJavaxSoundSampledSpiPart">
	</java-se-6:JavaxSoundSampledSpi>
	<java-se-6:JavaxSql rdf:about="&java-se-6;theJavaxSqlPart">
	</java-se-6:JavaxSql>
	<java-se-6:JavaxSqlRowset rdf:about="&java-se-6;theJavaxSqlRowsetPart">
	</java-se-6:JavaxSqlRowset>
	<java-se-6:JavaxSqlRowsetSpi rdf:about="&java-se-6;theJavaxSqlRowsetSpiPart">
	</java-se-6:JavaxSqlRowsetSpi>
	<java-se-6:JavaxSqlRowsetSerial rdf:about="&java-se-6;theJavaxSqlRowsetSerialPart">
	</java-se-6:JavaxSqlRowsetSerial>
	<java-se-6:JavaxTransaction rdf:about="&java-se-6;theJavaxTransactionPart">
	</java-se-6:JavaxTransaction>
	<java-se-6:JavaxTransactionXa rdf:about="&java-se-6;theJavaxTransactionXaPart">
	</java-se-6:JavaxTransactionXa>
	<java-se-6:JavaLang rdf:about="&java-se-6;theJavaLangPart">
	</java-se-6:JavaLang>
	<java-se-6:JavaLangAnnotation rdf:about="&java-se-6;theJavaLangAnnotationPart">
	</java-se-6:JavaLangAnnotation>
	<java-se-6:JavaLangReflect rdf:about="&java-se-6;theJavaLangReflectPart">
	</java-se-6:JavaLangReflect>
	<java-se-6:JavaLangInstrument rdf:about="&java-se-6;theJavaLangInstrumentPart">
	</java-se-6:JavaLangInstrument>
	<java-se-6:JavaLangManagement rdf:about="&java-se-6;theJavaLangManagementPart">
	</java-se-6:JavaLangManagement>
	<java-se-6:JavaLangRef rdf:about="&java-se-6;theJavaLangRefPart">
	</java-se-6:JavaLangRef>
	<java-se-6:JavaAwt rdf:about="&java-se-6;theJavaAwtPart">
	</java-se-6:JavaAwt>
	<java-se-6:JavaAwtPrint rdf:about="&java-se-6;theJavaAwtPrintPart">
	</java-se-6:JavaAwtPrint>
	<java-se-6:JavaAwtDatatransfer rdf:about="&java-se-6;theJavaAwtDatatransferPart">
	</java-se-6:JavaAwtDatatransfer>
	<java-se-6:JavaAwtEvent rdf:about="&java-se-6;theJavaAwtEventPart">
	</java-se-6:JavaAwtEvent>
	<java-se-6:JavaAwtImage rdf:about="&java-se-6;theJavaAwtImagePart">
	</java-se-6:JavaAwtImage>
	<java-se-6:JavaAwtImageRenderable rdf:about="&java-se-6;theJavaAwtImageRenderablePart">
	</java-se-6:JavaAwtImageRenderable>
	<java-se-6:JavaAwtGeom rdf:about="&java-se-6;theJavaAwtGeomPart">
	</java-se-6:JavaAwtGeom>
	<java-se-6:JavaAwtIm rdf:about="&java-se-6;theJavaAwtImPart">
	</java-se-6:JavaAwtIm>
	<java-se-6:JavaAwtImSpi rdf:about="&java-se-6;theJavaAwtImSpiPart">
	</java-se-6:JavaAwtImSpi>
	<java-se-6:JavaAwtColor rdf:about="&java-se-6;theJavaAwtColorPart">
	</java-se-6:JavaAwtColor>
	<java-se-6:JavaAwtDnd rdf:about="&java-se-6;theJavaAwtDndPart">
	</java-se-6:JavaAwtDnd>
	<java-se-6:JavaAwtFont rdf:about="&java-se-6;theJavaAwtFontPart">
	</java-se-6:JavaAwtFont>
	<java-se-6:JavaNet rdf:about="&java-se-6;theJavaNetPart">
	</java-se-6:JavaNet>
	<java-se-6:JavaIo rdf:about="&java-se-6;theJavaIoPart">
	</java-se-6:JavaIo>
	<java-se-6:JavaSecurity rdf:about="&java-se-6;theJavaSecurityPart">
	</java-se-6:JavaSecurity>
	<java-se-6:JavaSecuritySpec rdf:about="&java-se-6;theJavaSecuritySpecPart">
	</java-se-6:JavaSecuritySpec>
	<java-se-6:JavaSecurityCert rdf:about="&java-se-6;theJavaSecurityCertPart">
	</java-se-6:JavaSecurityCert>
	<java-se-6:JavaSecurityAcl rdf:about="&java-se-6;theJavaSecurityAclPart">
	</java-se-6:JavaSecurityAcl>
	<java-se-6:JavaSecurityInterfaces rdf:about="&java-se-6;theJavaSecurityInterfacesPart">
	</java-se-6:JavaSecurityInterfaces>
	<java-se-6:JavaMath rdf:about="&java-se-6;theJavaMathPart">
	</java-se-6:JavaMath>
	<java-se-6:JavaNio rdf:about="&java-se-6;theJavaNioPart">
	</java-se-6:JavaNio>
	<java-se-6:JavaNioChannels rdf:about="&java-se-6;theJavaNioChannelsPart">
	</java-se-6:JavaNioChannels>
	<java-se-6:JavaNioChannelsSpi rdf:about="&java-se-6;theJavaNioChannelsSpiPart">
	</java-se-6:JavaNioChannelsSpi>
	<java-se-6:JavaNioCharset rdf:about="&java-se-6;theJavaNioCharsetPart">
	</java-se-6:JavaNioCharset>
	<java-se-6:JavaNioCharsetSpi rdf:about="&java-se-6;theJavaNioCharsetSpiPart">
	</java-se-6:JavaNioCharsetSpi>
	<java-se-6:JavaUtil rdf:about="&java-se-6;theJavaUtilPart">
	</java-se-6:JavaUtil>
	<java-se-6:JavaUtilJar rdf:about="&java-se-6;theJavaUtilJarPart">
	</java-se-6:JavaUtilJar>
	<java-se-6:JavaUtilSpi rdf:about="&java-se-6;theJavaUtilSpiPart">
	</java-se-6:JavaUtilSpi>
	<java-se-6:JavaUtilConcurrent rdf:about="&java-se-6;theJavaUtilConcurrentPart">
	</java-se-6:JavaUtilConcurrent>
	<java-se-6:JavaUtilConcurrentAtomic rdf:about="&java-se-6;theJavaUtilConcurrentAtomicPart">
	</java-se-6:JavaUtilConcurrentAtomic>
	<java-se-6:JavaUtilConcurrentLocks rdf:about="&java-se-6;theJavaUtilConcurrentLocksPart">
	</java-se-6:JavaUtilConcurrentLocks>
	<java-se-6:JavaUtilZip rdf:about="&java-se-6;theJavaUtilZipPart">
	</java-se-6:JavaUtilZip>
	<java-se-6:JavaUtilLogging rdf:about="&java-se-6;theJavaUtilLoggingPart">
	</java-se-6:JavaUtilLogging>
	<java-se-6:JavaUtilPrefs rdf:about="&java-se-6;theJavaUtilPrefsPart">
	</java-se-6:JavaUtilPrefs>
	<java-se-6:JavaUtilRegex rdf:about="&java-se-6;theJavaUtilRegexPart">
	</java-se-6:JavaUtilRegex>
	<java-se-6:JavaApplet rdf:about="&java-se-6;theJavaAppletPart">
	</java-se-6:JavaApplet>
	<java-se-6:JavaBeans rdf:about="&java-se-6;theJavaBeansPart">
	</java-se-6:JavaBeans>
	<java-se-6:JavaBeansBeancontext rdf:about="&java-se-6;theJavaBeansBeancontextPart">
	</java-se-6:JavaBeansBeancontext>
	<java-se-6:JavaText rdf:about="&java-se-6;theJavaTextPart">
	</java-se-6:JavaText>
	<java-se-6:JavaTextSpi rdf:about="&java-se-6;theJavaTextSpiPart">
	</java-se-6:JavaTextSpi>
	<java-se-6:JavaRmi rdf:about="&java-se-6;theJavaRmiPart">
	</java-se-6:JavaRmi>
	<java-se-6:JavaRmiActivation rdf:about="&java-se-6;theJavaRmiActivationPart">
	</java-se-6:JavaRmiActivation>
	<java-se-6:JavaRmiServer rdf:about="&java-se-6;theJavaRmiServerPart">
	</java-se-6:JavaRmiServer>
	<java-se-6:JavaRmiDgc rdf:about="&java-se-6;theJavaRmiDgcPart">
	</java-se-6:JavaRmiDgc>
	<java-se-6:JavaRmiRegistry rdf:about="&java-se-6;theJavaRmiRegistryPart">
	</java-se-6:JavaRmiRegistry>
	<java-se-6:JavaSql rdf:about="&java-se-6;theJavaSqlPart">
	</java-se-6:JavaSql>
	<java-se-6:OrgW3cDom rdf:about="&java-se-6;theOrgW3cDomPart">
	</java-se-6:OrgW3cDom>
	<java-se-6:OrgW3cDomLs rdf:about="&java-se-6;theOrgW3cDomLsPart">
	</java-se-6:OrgW3cDomLs>
	<java-se-6:OrgW3cDomBootstrap rdf:about="&java-se-6;theOrgW3cDomBootstrapPart">
	</java-se-6:OrgW3cDomBootstrap>
	<java-se-6:OrgW3cDomCss rdf:about="&java-se-6;theOrgW3cDomCssPart">
	</java-se-6:OrgW3cDomCss>
	<java-se-6:OrgW3cDomStylesheets rdf:about="&java-se-6;theOrgW3cDomStylesheetsPart">
	</java-se-6:OrgW3cDomStylesheets>
	<java-se-6:OrgW3cDomViews rdf:about="&java-se-6;theOrgW3cDomViewsPart">
	</java-se-6:OrgW3cDomViews>
	<java-se-6:OrgW3cDomEvents rdf:about="&java-se-6;theOrgW3cDomEventsPart">
	</java-se-6:OrgW3cDomEvents>
	<java-se-6:OrgW3cDomHtml rdf:about="&java-se-6;theOrgW3cDomHtmlPart">
	</java-se-6:OrgW3cDomHtml>
	<java-se-6:OrgW3cDomTraversal rdf:about="&java-se-6;theOrgW3cDomTraversalPart">
	</java-se-6:OrgW3cDomTraversal>
	<java-se-6:OrgW3cDomRanges rdf:about="&java-se-6;theOrgW3cDomRangesPart">
	</java-se-6:OrgW3cDomRanges>
	<java-se-6:OrgW3cDomXpath rdf:about="&java-se-6;theOrgW3cDomXpathPart">
	</java-se-6:OrgW3cDomXpath>
	<java-se-6:OrgOmgCORBA_2_3 rdf:about="&java-se-6;theOrgOmgCORBA_2_3Part">
	</java-se-6:OrgOmgCORBA_2_3>
	<java-se-6:OrgOmgCORBA_2_3Portable rdf:about="&java-se-6;theOrgOmgCORBA_2_3PortablePart">
	</java-se-6:OrgOmgCORBA_2_3Portable>
	<java-se-6:OrgOmgCORBA rdf:about="&java-se-6;theOrgOmgCORBAPart">
	</java-se-6:OrgOmgCORBA>
	<java-se-6:OrgOmgCORBAPortable rdf:about="&java-se-6;theOrgOmgCORBAPortablePart">
	</java-se-6:OrgOmgCORBAPortable>
	<java-se-6:OrgOmgCORBADynAnyPackage rdf:about="&java-se-6;theOrgOmgCORBADynAnyPackagePart">
	</java-se-6:OrgOmgCORBADynAnyPackage>
	<java-se-6:OrgOmgCORBAORBPackage rdf:about="&java-se-6;theOrgOmgCORBAORBPackagePart">
	</java-se-6:OrgOmgCORBAORBPackage>
	<java-se-6:OrgOmgCORBATypeCodePackage rdf:about="&java-se-6;theOrgOmgCORBATypeCodePackagePart">
	</java-se-6:OrgOmgCORBATypeCodePackage>
	<java-se-6:OrgOmgSendingContext rdf:about="&java-se-6;theOrgOmgSendingContextPart">
	</java-se-6:OrgOmgSendingContext>
	<java-se-6:OrgOmgCosNaming rdf:about="&java-se-6;theOrgOmgCosNamingPart">
	</java-se-6:OrgOmgCosNaming>
	<java-se-6:OrgOmgCosNamingNamingContextExtPackage rdf:about="&java-se-6;theOrgOmgCosNamingNamingContextExtPackagePart">
	</java-se-6:OrgOmgCosNamingNamingContextExtPackage>
	<java-se-6:OrgOmgCosNamingNamingContextPackage rdf:about="&java-se-6;theOrgOmgCosNamingNamingContextPackagePart">
	</java-se-6:OrgOmgCosNamingNamingContextPackage>
	<java-se-6:OrgOmgPortableServer rdf:about="&java-se-6;theOrgOmgPortableServerPart">
	</java-se-6:OrgOmgPortableServer>
	<java-se-6:OrgOmgPortableServerCurrentPackage rdf:about="&java-se-6;theOrgOmgPortableServerCurrentPackagePart">
	</java-se-6:OrgOmgPortableServerCurrentPackage>
	<java-se-6:OrgOmgPortableServerPOAManagerPackage rdf:about="&java-se-6;theOrgOmgPortableServerPOAManagerPackagePart">
	</java-se-6:OrgOmgPortableServerPOAManagerPackage>
	<java-se-6:OrgOmgPortableServerPOAPackage rdf:about="&java-se-6;theOrgOmgPortableServerPOAPackagePart">
	</java-se-6:OrgOmgPortableServerPOAPackage>
	<java-se-6:OrgOmgPortableServerPortable rdf:about="&java-se-6;theOrgOmgPortableServerPortablePart">
	</java-se-6:OrgOmgPortableServerPortable>
	<java-se-6:OrgOmgPortableServerServantLocatorPackage rdf:about="&java-se-6;theOrgOmgPortableServerServantLocatorPackagePart">
	</java-se-6:OrgOmgPortableServerServantLocatorPackage>
	<java-se-6:OrgOmgDynamic rdf:about="&java-se-6;theOrgOmgDynamicPart">
	</java-se-6:OrgOmgDynamic>
	<java-se-6:OrgOmgDynamicAny rdf:about="&java-se-6;theOrgOmgDynamicAnyPart">
	</java-se-6:OrgOmgDynamicAny>
	<java-se-6:OrgOmgDynamicAnyDynAnyFactoryPackage rdf:about="&java-se-6;theOrgOmgDynamicAnyDynAnyFactoryPackagePart">
	</java-se-6:OrgOmgDynamicAnyDynAnyFactoryPackage>
	<java-se-6:OrgOmgDynamicAnyDynAnyPackage rdf:about="&java-se-6;theOrgOmgDynamicAnyDynAnyPackagePart">
	</java-se-6:OrgOmgDynamicAnyDynAnyPackage>
	<java-se-6:OrgOmgIOP rdf:about="&java-se-6;theOrgOmgIOPPart">
	</java-se-6:OrgOmgIOP>
	<java-se-6:OrgOmgIOPCodecFactoryPackage rdf:about="&java-se-6;theOrgOmgIOPCodecFactoryPackagePart">
	</java-se-6:OrgOmgIOPCodecFactoryPackage>
	<java-se-6:OrgOmgIOPCodecPackage rdf:about="&java-se-6;theOrgOmgIOPCodecPackagePart">
	</java-se-6:OrgOmgIOPCodecPackage>
	<java-se-6:OrgOmgMessaging rdf:about="&java-se-6;theOrgOmgMessagingPart">
	</java-se-6:OrgOmgMessaging>
	<java-se-6:OrgOmgPortableInterceptor rdf:about="&java-se-6;theOrgOmgPortableInterceptorPart">
	</java-se-6:OrgOmgPortableInterceptor>
	<java-se-6:OrgOmgPortableInterceptorORBInitInfoPackage rdf:about="&java-se-6;theOrgOmgPortableInterceptorORBInitInfoPackagePart">
	</java-se-6:OrgOmgPortableInterceptorORBInitInfoPackage>
	<java-se-6:OrgOmgStubJavaRmi rdf:about="&java-se-6;theOrgOmgStubJavaRmiPart">
	</java-se-6:OrgOmgStubJavaRmi>
	<java-se-6:OrgOmgStubJavaxManagementRemoteRmi rdf:about="&java-se-6;theOrgOmgStubJavaxManagementRemoteRmiPart">
	</java-se-6:OrgOmgStubJavaxManagementRemoteRmi>
	<java-se-6:OrgXmlSax rdf:about="&java-se-6;theOrgXmlSaxPart">
	</java-se-6:OrgXmlSax>
	<java-se-6:OrgXmlSaxHelpers rdf:about="&java-se-6;theOrgXmlSaxHelpersPart">
	</java-se-6:OrgXmlSaxHelpers>
	<java-se-6:OrgXmlSaxExt rdf:about="&java-se-6;theOrgXmlSaxExtPart">
	</java-se-6:OrgXmlSaxExt>
	<java-se-6:OrgIetfJgss rdf:about="&java-se-6;theOrgIetfJgssPart">
	</java-se-6:OrgIetfJgss>
	<owl:Class rdf:about="&java-se-6;JavaxJnlpClassLibrary">
		<rdfs:subClassOf rdf:resource="&java;JavaClassLibrary"/>
		<rdfs:comment xml:lang="en">JavaLibrary implementing the javax.jnlp package for Java SE 6</rdfs:comment>
		<rdfs:comment xml:lang="OWLManchester">platform:implementsInterface some JavaxJnlpAPI</rdfs:comment>
	</owl:Class>
	<owl:Class rdf:about="&java-se-6;JavaxCryptoClassLibrary">
		<owl:equivalentClass rdf:resource="&j2se-5_0;JavaxCryptoClassLibrary"/>
		<rdfs:subClassOf rdf:resource="&java;JavaClassLibrary"/>
		<rdfs:comment xml:lang="en">JavaLibrary implementing the javax.crypto package for Java SE 6</rdfs:comment>
		<rdfs:comment xml:lang="OWLManchester">platform:implementsInterface some JavaxCryptoAPI</rdfs:comment>
	</owl:Class>
	<owl:Class rdf:about="&java-se-6;JavaxCryptoInterfacesClassLibrary">
		<owl:equivalentClass rdf:resource="&j2se-5_0;JavaxCryptoInterfacesClassLibrary"/>
		<rdfs:subClassOf rdf:resource="&java;JavaClassLibrary"/>
		<rdfs:comment xml:lang="en">JavaLibrary implementing the javax.crypto.interfaces package for Java SE 6</rdfs:comment>
		<rdfs:comment xml:lang="OWLManchester">platform:implementsInterface some JavaxCryptoInterfacesAPI</rdfs:comment>
	</owl:Class>
	<owl:Class rdf:about="&java-se-6;JavaxCryptoSpecClassLibrary">
		<owl:equivalentClass rdf:resource="&j2se-5_0;JavaxCryptoSpecClassLibrary"/>
		<rdfs:subClassOf rdf:resource="&java;JavaClassLibrary"/>
		<rdfs:comment xml:lang="en">JavaLibrary implementing the javax.crypto.spec package for Java SE 6</rdfs:comment>
		<rdfs:comment xml:lang="OWLManchester">platform:implementsInterface some JavaxCryptoSpecAPI</rdfs:comment>
	</owl:Class>
	<owl:Class rdf:about="&java-se-6;JavaxNetClassLibrary">
		<owl:equivalentClass rdf:resource="&j2se-5_0;JavaxNetClassLibrary"/>
		<rdfs:subClassOf rdf:resource="&java;JavaClassLibrary"/>
		<rdfs:comment xml:lang="en">JavaLibrary implementing the javax.net package for Java SE 6</rdfs:comment>
		<rdfs:comment xml:lang="OWLManchester">platform:implementsInterface some JavaxNetAPI</rdfs:comment>
	</owl:Class>
	<owl:Class rdf:about="&java-se-6;JavaxNetSslClassLibrary">
		<rdfs:subClassOf rdf:resource="&j2se-5_0;JavaxNetSslClassLibrary"/>
		<rdfs:comment xml:lang="en">JavaLibrary implementing the javax.net.ssl package for Java SE 6</rdfs:comment>
		<rdfs:comment xml:lang="OWLManchester">platform:implementsInterface some JavaxNetSslAPI</rdfs:comment>
	</owl:Class>
	<owl:Class rdf:about="&java-se-6;JavaxSecurityCertClassLibrary">
		<owl:equivalentClass rdf:resource="&j2se-5_0;JavaxSecurityCertClassLibrary"/>
		<rdfs:subClassOf rdf:resource="&java;JavaClassLibrary"/>
		<rdfs:comment xml:lang="en">JavaLibrary implementing the javax.security.cert package for Java SE 6</rdfs:comment>
		<rdfs:comment xml:lang="OWLManchester">platform:implementsInterface some JavaxSecurityCertAPI</rdfs:comment>
	</owl:Class>
	<owl:Class rdf:about="&java-se-6;JavaxSecurityAuthClassLibrary">
		<owl:equivalentClass rdf:resource="&j2se-5_0;JavaxSecurityAuthClassLibrary"/>
		<rdfs:subClassOf rdf:resource="&java;JavaClassLibrary"/>
		<rdfs:comment xml:lang="en">JavaLibrary implementing the javax.security.auth package for Java SE 6</rdfs:comment>
		<rdfs:comment xml:lang="OWLManchester">platform:implementsInterface some JavaxSecurityAuthAPI</rdfs:comment>
	</owl:Class>
	<owl:Class rdf:about="&java-se-6;JavaxSecurityAuthCallbackClassLibrary">
		<owl:equivalentClass rdf:resource="&j2se-5_0;JavaxSecurityAuthCallbackClassLibrary"/>
		<rdfs:subClassOf rdf:resource="&java;JavaClassLibrary"/>
		<rdfs:comment xml:lang="en">JavaLibrary implementing the javax.security.auth.callback package for Java SE 6</rdfs:comment>
		<rdfs:comment xml:lang="OWLManchester">platform:implementsInterface some JavaxSecurityAuthCallbackAPI</rdfs:comment>
	</owl:Class>
	<owl:Class rdf:about="&java-se-6;JavaxSecurityAuthLoginClassLibrary">
		<rdfs:subClassOf rdf:resource="&j2se-5_0;JavaxSecurityAuthLoginClassLibrary"/>
		<rdfs:comment xml:lang="en">JavaLibrary implementing the javax.security.auth.login package for Java SE 6</rdfs:comment>
		<rdfs:comment xml:lang="OWLManchester">platform:implementsInterface some JavaxSecurityAuthLoginAPI</rdfs:comment>
	</owl:Class>
	<owl:Class rdf:about="&java-se-6;JavaxSecurityAuthX500ClassLibrary">
		<rdfs:subClassOf rdf:resource="&j2se-5_0;JavaxSecurityAuthX500ClassLibrary"/>
		<rdfs:comment xml:lang="en">JavaLibrary implementing the javax.security.auth.x500 package for Java SE 6</rdfs:comment>
		<rdfs:comment xml:lang="OWLManchester">platform:implementsInterface some JavaxSecurityAuthX500API</rdfs:comment>
	</owl:Class>
	<owl:Class rdf:about="&java-se-6;JavaxSecurityAuthKerberosClassLibrary">
		<owl:equivalentClass rdf:resource="&j2se-5_0;JavaxSecurityAuthKerberosClassLibrary"/>
		<rdfs:subClassOf rdf:resource="&java;JavaClassLibrary"/>
		<rdfs:comment xml:lang="en">JavaLibrary implementing the javax.security.auth.kerberos package for Java SE 6</rdfs:comment>
		<rdfs:comment xml:lang="OWLManchester">platform:implementsInterface some JavaxSecurityAuthKerberosAPI</rdfs:comment>
	</owl:Class>
	<owl:Class rdf:about="&java-se-6;JavaxSecurityAuthSpiClassLibrary">
		<owl:equivalentClass rdf:resource="&j2se-5_0;JavaxSecurityAuthSpiClassLibrary"/>
		<rdfs:subClassOf rdf:resource="&java;JavaClassLibrary"/>
		<rdfs:comment xml:lang="en">JavaLibrary implementing the javax.security.auth.spi package for Java SE 6</rdfs:comment>
		<rdfs:comment xml:lang="OWLManchester">platform:implementsInterface some JavaxSecurityAuthSpiAPI</rdfs:comment>
	</owl:Class>
	<owl:Class rdf:about="&java-se-6;JavaxSecuritySaslClassLibrary">
		<rdfs:subClassOf rdf:resource="&j2se-5_0;JavaxSecuritySaslClassLibrary"/>
		<rdfs:comment xml:lang="en">JavaLibrary implementing the javax.security.sasl package for Java SE 6</rdfs:comment>
		<rdfs:comment xml:lang="OWLManchester">platform:implementsInterface some JavaxSecuritySaslAPI</rdfs:comment>
	</owl:Class>
	<owl:Class rdf:about="&java-se-6;JavaxAccessibilityClassLibrary">
		<rdfs:subClassOf rdf:resource="&j2se-5_0;JavaxAccessibilityClassLibrary"/>
		<rdfs:comment xml:lang="en">JavaLibrary implementing the javax.accessibility package for Java SE 6</rdfs:comment>
		<rdfs:comment xml:lang="OWLManchester">platform:implementsInterface some JavaxAccessibilityAPI</rdfs:comment>
	</owl:Class>
	<owl:Class rdf:about="&java-se-6;JavaxSwingClassLibrary">
		<rdfs:subClassOf rdf:resource="&j2se-5_0;JavaxSwingClassLibrary"/>
		<rdfs:comment xml:lang="en">JavaLibrary implementing the javax.swing package for Java SE 6</rdfs:comment>
		<rdfs:comment xml:lang="OWLManchester">platform:implementsInterface some JavaxSwingAPI</rdfs:comment>
	</owl:Class>
	<owl:Class rdf:about="&java-se-6;JavaxSwingTextClassLibrary">
		<rdfs:subClassOf rdf:resource="&j2se-5_0;JavaxSwingTextClassLibrary"/>
		<rdfs:comment xml:lang="en">JavaLibrary implementing the javax.swing.text package for Java SE 6</rdfs:comment>
		<rdfs:comment xml:lang="OWLManchester">platform:implementsInterface some JavaxSwingTextAPI</rdfs:comment>
	</owl:Class>
	<owl:Class rdf:about="&java-se-6;JavaxSwingTextHtmlClassLibrary">
		<rdfs:subClassOf rdf:resource="&j2se-5_0;JavaxSwingTextHtmlClassLibrary"/>
		<rdfs:comment xml:lang="en">JavaLibrary implementing the javax.swing.text.html package for Java SE 6</rdfs:comment>
		<rdfs:comment xml:lang="OWLManchester">platform:implementsInterface some JavaxSwingTextHtmlAPI</rdfs:comment>
	</owl:Class>
	<owl:Class rdf:about="&java-se-6;JavaxSwingTextHtmlParserClassLibrary">
		<owl:equivalentClass rdf:resource="&j2se-5_0;JavaxSwingTextHtmlParserClassLibrary"/>
		<rdfs:subClassOf rdf:resource="&java;JavaClassLibrary"/>
		<rdfs:comment xml:lang="en">JavaLibrary implementing the javax.swing.text.html.parser package for Java SE 6</rdfs:comment>
		<rdfs:comment xml:lang="OWLManchester">platform:implementsInterface some JavaxSwingTextHtmlParserAPI</rdfs:comment>
	</owl:Class>
	<owl:Class rdf:about="&java-se-6;JavaxSwingTextRtfClassLibrary">
		<rdfs:subClassOf rdf:resource="&j2se-5_0;JavaxSwingTextRtfClassLibrary"/>
		<rdfs:comment xml:lang="en">JavaLibrary implementing the javax.swing.text.rtf package for Java SE 6</rdfs:comment>
		<rdfs:comment xml:lang="OWLManchester">platform:implementsInterface some JavaxSwingTextRtfAPI</rdfs:comment>
	</owl:Class>
	<owl:Class rdf:about="&java-se-6;JavaxSwingEventClassLibrary">
		<rdfs:subClassOf rdf:resource="&j2se-5_0;JavaxSwingEventClassLibrary"/>
		<rdfs:comment xml:lang="en">JavaLibrary implementing the javax.swing.event package for Java SE 6</rdfs:comment>
		<rdfs:comment xml:lang="OWLManchester">platform:implementsInterface some JavaxSwingEventAPI</rdfs:comment>
	</owl:Class>
	<owl:Class rdf:about="&java-se-6;JavaxSwingColorchooserClassLibrary">
		<rdfs:subClassOf rdf:resource="&j2se-5_0;JavaxSwingColorchooserClassLibrary"/>
		<rdfs:comment xml:lang="en">JavaLibrary implementing the javax.swing.colorchooser package for Java SE 6</rdfs:comment>
		<rdfs:comment xml:lang="OWLManchester">platform:implementsInterface some JavaxSwingColorchooserAPI</rdfs:comment>
	</owl:Class>
	<owl:Class rdf:about="&java-se-6;JavaxSwingPlafClassLibrary">
		<rdfs:subClassOf rdf:resource="&j2se-5_0;JavaxSwingPlafClassLibrary"/>
		<rdfs:comment xml:lang="en">JavaLibrary implementing the javax.swing.plaf package for Java SE 6</rdfs:comment>
		<rdfs:comment xml:lang="OWLManchester">platform:implementsInterface some JavaxSwingPlafAPI</rdfs:comment>
	</owl:Class>
	<owl:Class rdf:about="&java-se-6;JavaxSwingPlafBasicClassLibrary">
		<rdfs:subClassOf rdf:resource="&j2se-5_0;JavaxSwingPlafBasicClassLibrary"/>
		<rdfs:comment xml:lang="en">JavaLibrary implementing the javax.swing.plaf.basic package for Java SE 6</rdfs:comment>
		<rdfs:comment xml:lang="OWLManchester">platform:implementsInterface some JavaxSwingPlafBasicAPI</rdfs:comment>
	</owl:Class>
	<owl:Class rdf:about="&java-se-6;JavaxSwingPlafMetalClassLibrary">
		<rdfs:subClassOf rdf:resource="&j2se-5_0;JavaxSwingPlafMetalClassLibrary"/>
		<rdfs:comment xml:lang="en">JavaLibrary implementing the javax.swing.plaf.metal package for Java SE 6</rdfs:comment>
		<rdfs:comment xml:lang="OWLManchester">platform:implementsInterface some JavaxSwingPlafMetalAPI</rdfs:comment>
	</owl:Class>
	<owl:Class rdf:about="&java-se-6;JavaxSwingPlafMultiClassLibrary">
		<rdfs:subClassOf rdf:resource="&j2se-5_0;JavaxSwingPlafMultiClassLibrary"/>
		<rdfs:comment xml:lang="en">JavaLibrary implementing the javax.swing.plaf.multi package for Java SE 6</rdfs:comment>
		<rdfs:comment xml:lang="OWLManchester">platform:implementsInterface some JavaxSwingPlafMultiAPI</rdfs:comment>
	</owl:Class>
	<owl:Class rdf:about="&java-se-6;JavaxSwingPlafSynthClassLibrary">
		<rdfs:subClassOf rdf:resource="&j2se-5_0;JavaxSwingPlafSynthClassLibrary"/>
		<rdfs:comment xml:lang="en">JavaLibrary implementing the javax.swing.plaf.synth package for Java SE 6</rdfs:comment>
		<rdfs:comment xml:lang="OWLManchester">platform:implementsInterface some JavaxSwingPlafSynthAPI</rdfs:comment>
	</owl:Class>
	<owl:Class rdf:about="&java-se-6;JavaxSwingFilechooserClassLibrary">
		<rdfs:subClassOf rdf:resource="&j2se-5_0;JavaxSwingFilechooserClassLibrary"/>
		<rdfs:comment xml:lang="en">JavaLibrary implementing the javax.swing.filechooser package for Java SE 6</rdfs:comment>
		<rdfs:comment xml:lang="OWLManchester">platform:implementsInterface some JavaxSwingFilechooserAPI</rdfs:comment>
	</owl:Class>
	<owl:Class rdf:about="&java-se-6;JavaxSwingTreeClassLibrary">
		<rdfs:subClassOf rdf:resource="&j2se-5_0;JavaxSwingTreeClassLibrary"/>
		<rdfs:comment xml:lang="en">JavaLibrary implementing the javax.swing.tree package for Java SE 6</rdfs:comment>
		<rdfs:comment xml:lang="OWLManchester">platform:implementsInterface some JavaxSwingTreeAPI</rdfs:comment>
	</owl:Class>
	<owl:Class rdf:about="&java-se-6;JavaxSwingBorderClassLibrary">
		<rdfs:subClassOf rdf:resource="&j2se-5_0;JavaxSwingBorderClassLibrary"/>
		<rdfs:comment xml:lang="en">JavaLibrary implementing the javax.swing.border package for Java SE 6</rdfs:comment>
		<rdfs:comment xml:lang="OWLManchester">platform:implementsInterface some JavaxSwingBorderAPI</rdfs:comment>
	</owl:Class>
	<owl:Class rdf:about="&java-se-6;JavaxSwingTableClassLibrary">
		<rdfs:subClassOf rdf:resource="&j2se-5_0;JavaxSwingTableClassLibrary"/>
		<rdfs:comment xml:lang="en">JavaLibrary implementing the javax.swing.table package for Java SE 6</rdfs:comment>
		<rdfs:comment xml:lang="OWLManchester">platform:implementsInterface some JavaxSwingTableAPI</rdfs:comment>
	</owl:Class>
	<owl:Class rdf:about="&java-se-6;JavaxSwingUndoClassLibrary">
		<owl:equivalentClass rdf:resource="&j2se-5_0;JavaxSwingUndoClassLibrary"/>
		<rdfs:subClassOf rdf:resource="&java;JavaClassLibrary"/>
		<rdfs:comment xml:lang="en">JavaLibrary implementing the javax.swing.undo package for Java SE 6</rdfs:comment>
		<rdfs:comment xml:lang="OWLManchester">platform:implementsInterface some JavaxSwingUndoAPI</rdfs:comment>
	</owl:Class>
	<owl:Class rdf:about="&java-se-6;JavaxManagementClassLibrary">
		<rdfs:subClassOf rdf:resource="&j2se-5_0;JavaxManagementClassLibrary"/>
		<rdfs:comment xml:lang="en">JavaLibrary implementing the javax.management package for Java SE 6</rdfs:comment>
		<rdfs:comment xml:lang="OWLManchester">platform:implementsInterface some JavaxManagementAPI</rdfs:comment>
	</owl:Class>
	<owl:Class rdf:about="&java-se-6;JavaxManagementOpenmbeanClassLibrary">
		<rdfs:subClassOf rdf:resource="&j2se-5_0;JavaxManagementOpenmbeanClassLibrary"/>
		<rdfs:comment xml:lang="en">JavaLibrary implementing the javax.management.openmbean package for Java SE 6</rdfs:comment>
		<rdfs:comment xml:lang="OWLManchester">platform:implementsInterface some JavaxManagementOpenmbeanAPI</rdfs:comment>
	</owl:Class>
	<owl:Class rdf:about="&java-se-6;JavaxManagementLoadingClassLibrary">
		<rdfs:subClassOf rdf:resource="&j2se-5_0;JavaxManagementLoadingClassLibrary"/>
		<rdfs:comment xml:lang="en">JavaLibrary implementing the javax.management.loading package for Java SE 6</rdfs:comment>
		<rdfs:comment xml:lang="OWLManchester">platform:implementsInterface some JavaxManagementLoadingAPI</rdfs:comment>
	</owl:Class>
	<owl:Class rdf:about="&java-se-6;JavaxManagementModelmbeanClassLibrary">
		<rdfs:subClassOf rdf:resource="&j2se-5_0;JavaxManagementModelmbeanClassLibrary"/>
		<rdfs:comment xml:lang="en">JavaLibrary implementing the javax.management.modelmbean package for Java SE 6</rdfs:comment>
		<rdfs:comment xml:lang="OWLManchester">platform:implementsInterface some JavaxManagementModelmbeanAPI</rdfs:comment>
	</owl:Class>
	<owl:Class rdf:about="&java-se-6;JavaxManagementMonitorClassLibrary">
		<rdfs:subClassOf rdf:resource="&j2se-5_0;JavaxManagementMonitorClassLibrary"/>
		<rdfs:comment xml:lang="en">JavaLibrary implementing the javax.management.monitor package for Java SE 6</rdfs:comment>
		<rdfs:comment xml:lang="OWLManchester">platform:implementsInterface some JavaxManagementMonitorAPI</rdfs:comment>
	</owl:Class>
	<owl:Class rdf:about="&java-se-6;JavaxManagementRelationClassLibrary">
		<rdfs:subClassOf rdf:resource="&j2se-5_0;JavaxManagementRelationClassLibrary"/>
		<rdfs:comment xml:lang="en">JavaLibrary implementing the javax.management.relation package for Java SE 6</rdfs:comment>
		<rdfs:comment xml:lang="OWLManchester">platform:implementsInterface some JavaxManagementRelationAPI</rdfs:comment>
	</owl:Class>
	<owl:Class rdf:about="&java-se-6;JavaxManagementRemoteClassLibrary">
		<rdfs:subClassOf rdf:resource="&j2se-5_0;JavaxManagementRemoteClassLibrary"/>
		<rdfs:comment xml:lang="en">JavaLibrary implementing the javax.management.remote package for Java SE 6</rdfs:comment>
		<rdfs:comment xml:lang="OWLManchester">platform:implementsInterface some JavaxManagementRemoteAPI</rdfs:comment>
	</owl:Class>
	<owl:Class rdf:about="&java-se-6;JavaxManagementRemoteRmiClassLibrary">
		<rdfs:subClassOf rdf:resource="&j2se-5_0;JavaxManagementRemoteRmiClassLibrary"/>
		<rdfs:comment xml:lang="en">JavaLibrary implementing the javax.management.remote.rmi package for Java SE 6</rdfs:comment>
		<rdfs:comment xml:lang="OWLManchester">platform:implementsInterface some JavaxManagementRemoteRmiAPI</rdfs:comment>
	</owl:Class>
	<owl:Class rdf:about="&java-se-6;JavaxManagementTimerClassLibrary">
		<rdfs:subClassOf rdf:resource="&java;JavaClassLibrary"/>
		<rdfs:comment xml:lang="en">JavaLibrary implementing the javax.management.timer package for Java SE 6</rdfs:comment>
		<rdfs:comment xml:lang="OWLManchester">platform:implementsInterface some JavaxManagementTimerAPI</rdfs:comment>
	</owl:Class>
	<owl:Class rdf:about="&java-se-6;JavaxXmlClassLibrary">
		<owl:equivalentClass rdf:resource="&j2se-5_0;JavaxXmlClassLibrary"/>
		<rdfs:subClassOf rdf:resource="&java;JavaClassLibrary"/>
		<rdfs:comment xml:lang="en">JavaLibrary implementing the javax.xml package for Java SE 6</rdfs:comment>
		<rdfs:comment xml:lang="OWLManchester">platform:implementsInterface some JavaxXmlAPI</rdfs:comment>
	</owl:Class>
	<owl:Class rdf:about="&java-se-6;JavaxXmlTransformClassLibrary">
		<rdfs:subClassOf rdf:resource="&j2se-5_0;JavaxXmlTransformClassLibrary"/>
		<rdfs:comment xml:lang="en">JavaLibrary implementing the javax.xml.transform package for Java SE 6</rdfs:comment>
		<rdfs:comment xml:lang="OWLManchester">platform:implementsInterface some JavaxXmlTransformAPI</rdfs:comment>
	</owl:Class>
	<owl:Class rdf:about="&java-se-6;JavaxXmlTransformDomClassLibrary">
		<owl:equivalentClass rdf:resource="&j2se-5_0;JavaxXmlTransformDomClassLibrary"/>
		<rdfs:subClassOf rdf:resource="&java;JavaClassLibrary"/>
		<rdfs:comment xml:lang="en">JavaLibrary implementing the javax.xml.transform.dom package for Java SE 6</rdfs:comment>
		<rdfs:comment xml:lang="OWLManchester">platform:implementsInterface some JavaxXmlTransformDomAPI</rdfs:comment>
	</owl:Class>
	<owl:Class rdf:about="&java-se-6;JavaxXmlTransformSaxClassLibrary">
		<rdfs:subClassOf rdf:resource="&j2se-5_0;JavaxXmlTransformSaxClassLibrary"/>
		<rdfs:comment xml:lang="en">JavaLibrary implementing the javax.xml.transform.sax package for Java SE 6</rdfs:comment>
		<rdfs:comment xml:lang="OWLManchester">platform:implementsInterface some JavaxXmlTransformSaxAPI</rdfs:comment>
	</owl:Class>
	<owl:Class rdf:about="&java-se-6;JavaxXmlTransformStaxClassLibrary">
		<rdfs:subClassOf rdf:resource="&java;JavaClassLibrary"/>
		<rdfs:comment xml:lang="en">JavaLibrary implementing the javax.xml.transform.stax package for Java SE 6</rdfs:comment>
		<rdfs:comment xml:lang="OWLManchester">platform:implementsInterface some JavaxXmlTransformStaxAPI</rdfs:comment>
	</owl:Class>
	<owl:Class rdf:about="&java-se-6;JavaxXmlTransformStreamClassLibrary">
		<owl:equivalentClass rdf:resource="&j2se-5_0;JavaxXmlTransformStreamClassLibrary"/>
		<rdfs:subClassOf rdf:resource="&java;JavaClassLibrary"/>
		<rdfs:comment xml:lang="en">JavaLibrary implementing the javax.xml.transform.stream package for Java SE 6</rdfs:comment>
		<rdfs:comment xml:lang="OWLManchester">platform:implementsInterface some JavaxXmlTransformStreamAPI</rdfs:comment>
	</owl:Class>
	<owl:Class rdf:about="&java-se-6;JavaxXmlBindClassLibrary">
		<rdfs:subClassOf rdf:resource="&java;JavaClassLibrary"/>
		<rdfs:comment xml:lang="en">JavaLibrary implementing the javax.xml.bind package for Java SE 6</rdfs:comment>
		<rdfs:comment xml:lang="OWLManchester">platform:implementsInterface some JavaxXmlBindAPI</rdfs:comment>
	</owl:Class>
	<owl:Class rdf:about="&java-se-6;JavaxXmlBindAnnotationClassLibrary">
		<rdfs:subClassOf rdf:resource="&java;JavaClassLibrary"/>
		<rdfs:comment xml:lang="en">JavaLibrary implementing the javax.xml.bind.annotation package for Java SE 6</rdfs:comment>
		<rdfs:comment xml:lang="OWLManchester">platform:implementsInterface some JavaxXmlBindAnnotationAPI</rdfs:comment>
	</owl:Class>
	<owl:Class rdf:about="&java-se-6;JavaxXmlBindAnnotationAdaptersClassLibrary">
		<rdfs:subClassOf rdf:resource="&java;JavaClassLibrary"/>
		<rdfs:comment xml:lang="en">JavaLibrary implementing the javax.xml.bind.annotation.adapters package for Java SE 6</rdfs:comment>
		<rdfs:comment xml:lang="OWLManchester">platform:implementsInterface some JavaxXmlBindAnnotationAdaptersAPI</rdfs:comment>
	</owl:Class>
	<owl:Class rdf:about="&java-se-6;JavaxXmlBindAttachmentClassLibrary">
		<rdfs:subClassOf rdf:resource="&java;JavaClassLibrary"/>
		<rdfs:comment xml:lang="en">JavaLibrary implementing the javax.xml.bind.attachment package for Java SE 6</rdfs:comment>
		<rdfs:comment xml:lang="OWLManchester">platform:implementsInterface some JavaxXmlBindAttachmentAPI</rdfs:comment>
	</owl:Class>
	<owl:Class rdf:about="&java-se-6;JavaxXmlBindHelpersClassLibrary">
		<rdfs:subClassOf rdf:resource="&java;JavaClassLibrary"/>
		<rdfs:comment xml:lang="en">JavaLibrary implementing the javax.xml.bind.helpers package for Java SE 6</rdfs:comment>
		<rdfs:comment xml:lang="OWLManchester">platform:implementsInterface some JavaxXmlBindHelpersAPI</rdfs:comment>
	</owl:Class>
	<owl:Class rdf:about="&java-se-6;JavaxXmlBindUtilClassLibrary">
		<rdfs:subClassOf rdf:resource="&java;JavaClassLibrary"/>
		<rdfs:comment xml:lang="en">JavaLibrary implementing the javax.xml.bind.util package for Java SE 6</rdfs:comment>
		<rdfs:comment xml:lang="OWLManchester">platform:implementsInterface some JavaxXmlBindUtilAPI</rdfs:comment>
	</owl:Class>
	<owl:Class rdf:about="&java-se-6;JavaxXmlValidationClassLibrary">
		<rdfs:subClassOf rdf:resource="&j2se-5_0;JavaxXmlValidationClassLibrary"/>
		<rdfs:comment xml:lang="en">JavaLibrary implementing the javax.xml.validation package for Java SE 6</rdfs:comment>
		<rdfs:comment xml:lang="OWLManchester">platform:implementsInterface some JavaxXmlValidationAPI</rdfs:comment>
	</owl:Class>
	<owl:Class rdf:about="&java-se-6;JavaxXmlNamespaceClassLibrary">
		<owl:equivalentClass rdf:resource="&j2se-5_0;JavaxXmlNamespaceClassLibrary"/>
		<rdfs:subClassOf rdf:resource="&java;JavaClassLibrary"/>
		<rdfs:comment xml:lang="en">JavaLibrary implementing the javax.xml.namespace package for Java SE 6</rdfs:comment>
		<rdfs:comment xml:lang="OWLManchester">platform:implementsInterface some JavaxXmlNamespaceAPI</rdfs:comment>
	</owl:Class>
	<owl:Class rdf:about="&java-se-6;JavaxXmlStreamClassLibrary">
		<rdfs:subClassOf rdf:resource="&java;JavaClassLibrary"/>
		<rdfs:comment xml:lang="en">JavaLibrary implementing the javax.xml.stream package for Java SE 6</rdfs:comment>
		<rdfs:comment xml:lang="OWLManchester">platform:implementsInterface some JavaxXmlStreamAPI</rdfs:comment>
	</owl:Class>
	<owl:Class rdf:about="&java-se-6;JavaxXmlStreamEventsClassLibrary">
		<rdfs:subClassOf rdf:resource="&java;JavaClassLibrary"/>
		<rdfs:comment xml:lang="en">JavaLibrary implementing the javax.xml.stream.events package for Java SE 6</rdfs:comment>
		<rdfs:comment xml:lang="OWLManchester">platform:implementsInterface some JavaxXmlStreamEventsAPI</rdfs:comment>
	</owl:Class>
	<owl:Class rdf:about="&java-se-6;JavaxXmlStreamUtilClassLibrary">
		<rdfs:subClassOf rdf:resource="&java;JavaClassLibrary"/>
		<rdfs:comment xml:lang="en">JavaLibrary implementing the javax.xml.stream.util package for Java SE 6</rdfs:comment>
		<rdfs:comment xml:lang="OWLManchester">platform:implementsInterface some JavaxXmlStreamUtilAPI</rdfs:comment>
	</owl:Class>
	<owl:Class rdf:about="&java-se-6;JavaxXmlParsersClassLibrary">
		<rdfs:subClassOf rdf:resource="&j2se-5_0;JavaxXmlParsersClassLibrary"/>
		<rdfs:comment xml:lang="en">JavaLibrary implementing the javax.xml.parsers package for Java SE 6</rdfs:comment>
		<rdfs:comment xml:lang="OWLManchester">platform:implementsInterface some JavaxXmlParsersAPI</rdfs:comment>
	</owl:Class>
	<owl:Class rdf:about="&java-se-6;JavaxXmlCryptoClassLibrary">
		<rdfs:subClassOf rdf:resource="&java;JavaClassLibrary"/>
		<rdfs:comment xml:lang="en">JavaLibrary implementing the javax.xml.crypto package for Java SE 6</rdfs:comment>
		<rdfs:comment xml:lang="OWLManchester">platform:implementsInterface some JavaxXmlCryptoAPI</rdfs:comment>
	</owl:Class>
	<owl:Class rdf:about="&java-se-6;JavaxXmlCryptoDsigClassLibrary">
		<rdfs:subClassOf rdf:resource="&java;JavaClassLibrary"/>
		<rdfs:comment xml:lang="en">JavaLibrary implementing the javax.xml.crypto.dsig package for Java SE 6</rdfs:comment>
		<rdfs:comment xml:lang="OWLManchester">platform:implementsInterface some JavaxXmlCryptoDsigAPI</rdfs:comment>
	</owl:Class>
	<owl:Class rdf:about="&java-se-6;JavaxXmlCryptoDsigKeyinfoClassLibrary">
		<rdfs:subClassOf rdf:resource="&java;JavaClassLibrary"/>
		<rdfs:comment xml:lang="en">JavaLibrary implementing the javax.xml.crypto.dsig.keyinfo package for Java SE 6</rdfs:comment>
		<rdfs:comment xml:lang="OWLManchester">platform:implementsInterface some JavaxXmlCryptoDsigKeyinfoAPI</rdfs:comment>
	</owl:Class>
	<owl:Class rdf:about="&java-se-6;JavaxXmlCryptoDsigSpecClassLibrary">
		<rdfs:subClassOf rdf:resource="&java;JavaClassLibrary"/>
		<rdfs:comment xml:lang="en">JavaLibrary implementing the javax.xml.crypto.dsig.spec package for Java SE 6</rdfs:comment>
		<rdfs:comment xml:lang="OWLManchester">platform:implementsInterface some JavaxXmlCryptoDsigSpecAPI</rdfs:comment>
	</owl:Class>
	<owl:Class rdf:about="&java-se-6;JavaxXmlCryptoDsigDomClassLibrary">
		<rdfs:subClassOf rdf:resource="&java;JavaClassLibrary"/>
		<rdfs:comment xml:lang="en">JavaLibrary implementing the javax.xml.crypto.dsig.dom package for Java SE 6</rdfs:comment>
		<rdfs:comment xml:lang="OWLManchester">platform:implementsInterface some JavaxXmlCryptoDsigDomAPI</rdfs:comment>
	</owl:Class>
	<owl:Class rdf:about="&java-se-6;JavaxXmlCryptoDomClassLibrary">
		<rdfs:subClassOf rdf:resource="&java;JavaClassLibrary"/>
		<rdfs:comment xml:lang="en">JavaLibrary implementing the javax.xml.crypto.dom package for Java SE 6</rdfs:comment>
		<rdfs:comment xml:lang="OWLManchester">platform:implementsInterface some JavaxXmlCryptoDomAPI</rdfs:comment>
	</owl:Class>
	<owl:Class rdf:about="&java-se-6;JavaxXmlDatatypeClassLibrary">
		<rdfs:subClassOf rdf:resource="&j2se-5_0;JavaxXmlDatatypeClassLibrary"/>
		<rdfs:comment xml:lang="en">JavaLibrary implementing the javax.xml.datatype package for Java SE 6</rdfs:comment>
		<rdfs:comment xml:lang="OWLManchester">platform:implementsInterface some JavaxXmlDatatypeAPI</rdfs:comment>
	</owl:Class>
	<owl:Class rdf:about="&java-se-6;JavaxXmlSoapClassLibrary">
		<rdfs:subClassOf rdf:resource="&java;JavaClassLibrary"/>
		<rdfs:comment xml:lang="en">JavaLibrary implementing the javax.xml.soap package for Java SE 6</rdfs:comment>
		<rdfs:comment xml:lang="OWLManchester">platform:implementsInterface some JavaxXmlSoapAPI</rdfs:comment>
	</owl:Class>
	<owl:Class rdf:about="&java-se-6;JavaxXmlWsClassLibrary">
		<rdfs:subClassOf rdf:resource="&java;JavaClassLibrary"/>
		<rdfs:comment xml:lang="en">JavaLibrary implementing the javax.xml.ws package for Java SE 6</rdfs:comment>
		<rdfs:comment xml:lang="OWLManchester">platform:implementsInterface some JavaxXmlWsAPI</rdfs:comment>
	</owl:Class>
	<owl:Class rdf:about="&java-se-6;JavaxXmlWsHandlerClassLibrary">
		<rdfs:subClassOf rdf:resource="&java;JavaClassLibrary"/>
		<rdfs:comment xml:lang="en">JavaLibrary implementing the javax.xml.ws.handler package for Java SE 6</rdfs:comment>
		<rdfs:comment xml:lang="OWLManchester">platform:implementsInterface some JavaxXmlWsHandlerAPI</rdfs:comment>
	</owl:Class>
	<owl:Class rdf:about="&java-se-6;JavaxXmlWsHandlerSoapClassLibrary">
		<rdfs:subClassOf rdf:resource="&java;JavaClassLibrary"/>
		<rdfs:comment xml:lang="en">JavaLibrary implementing the javax.xml.ws.handler.soap package for Java SE 6</rdfs:comment>
		<rdfs:comment xml:lang="OWLManchester">platform:implementsInterface some JavaxXmlWsHandlerSoapAPI</rdfs:comment>
	</owl:Class>
	<owl:Class rdf:about="&java-se-6;JavaxXmlWsHttpClassLibrary">
		<rdfs:subClassOf rdf:resource="&java;JavaClassLibrary"/>
		<rdfs:comment xml:lang="en">JavaLibrary implementing the javax.xml.ws.http package for Java SE 6</rdfs:comment>
		<rdfs:comment xml:lang="OWLManchester">platform:implementsInterface some JavaxXmlWsHttpAPI</rdfs:comment>
	</owl:Class>
	<owl:Class rdf:about="&java-se-6;JavaxXmlWsSoapClassLibrary">
		<rdfs:subClassOf rdf:resource="&java;JavaClassLibrary"/>
		<rdfs:comment xml:lang="en">JavaLibrary implementing the javax.xml.ws.soap package for Java SE 6</rdfs:comment>
		<rdfs:comment xml:lang="OWLManchester">platform:implementsInterface some JavaxXmlWsSoapAPI</rdfs:comment>
	</owl:Class>
	<owl:Class rdf:about="&java-se-6;JavaxXmlWsSpiClassLibrary">
		<rdfs:subClassOf rdf:resource="&java;JavaClassLibrary"/>
		<rdfs:comment xml:lang="en">JavaLibrary implementing the javax.xml.ws.spi package for Java SE 6</rdfs:comment>
		<rdfs:comment xml:lang="OWLManchester">platform:implementsInterface some JavaxXmlWsSpiAPI</rdfs:comment>
	</owl:Class>
	<owl:Class rdf:about="&java-se-6;JavaxXmlWsWsaddressingClassLibrary">
		<rdfs:subClassOf rdf:resource="&java;JavaClassLibrary"/>
		<rdfs:comment xml:lang="en">JavaLibrary implementing the javax.xml.ws.wsaddressing package for Java SE 6</rdfs:comment>
		<rdfs:comment xml:lang="OWLManchester">platform:implementsInterface some JavaxXmlWsWsaddressingAPI</rdfs:comment>
	</owl:Class>
	<owl:Class rdf:about="&java-se-6;JavaxXmlXpathClassLibrary">
		<rdfs:subClassOf rdf:resource="&j2se-5_0;JavaxXmlXpathClassLibrary"/>
		<rdfs:comment xml:lang="en">JavaLibrary implementing the javax.xml.xpath package for Java SE 6</rdfs:comment>
		<rdfs:comment xml:lang="OWLManchester">platform:implementsInterface some JavaxXmlXpathAPI</rdfs:comment>
	</owl:Class>
	<owl:Class rdf:about="&java-se-6;JavaxActivationClassLibrary">
		<rdfs:subClassOf rdf:resource="&java;JavaClassLibrary"/>
		<rdfs:comment xml:lang="en">JavaLibrary implementing the javax.activation package for Java SE 6</rdfs:comment>
		<rdfs:comment xml:lang="OWLManchester">platform:implementsInterface some JavaxActivationAPI</rdfs:comment>
	</owl:Class>
	<owl:Class rdf:about="&java-se-6;JavaxActivityClassLibrary">
		<owl:equivalentClass rdf:resource="&j2se-5_0;JavaxActivityClassLibrary"/>
		<rdfs:subClassOf rdf:resource="&java;JavaClassLibrary"/>
		<rdfs:comment xml:lang="en">JavaLibrary implementing the javax.activity package for Java SE 6</rdfs:comment>
		<rdfs:comment xml:lang="OWLManchester">platform:implementsInterface some JavaxActivityAPI</rdfs:comment>
	</owl:Class>
	<owl:Class rdf:about="&java-se-6;JavaxAnnotationClassLibrary">
		<rdfs:subClassOf rdf:resource="&java;JavaClassLibrary"/>
		<rdfs:comment xml:lang="en">JavaLibrary implementing the javax.annotation package for Java SE 6</rdfs:comment>
		<rdfs:comment xml:lang="OWLManchester">platform:implementsInterface some JavaxAnnotationAPI</rdfs:comment>
	</owl:Class>
	<owl:Class rdf:about="&java-se-6;JavaxAnnotationProcessingClassLibrary">
		<rdfs:subClassOf rdf:resource="&java;JavaClassLibrary"/>
		<rdfs:comment xml:lang="en">JavaLibrary implementing the javax.annotation.processing package for Java SE 6</rdfs:comment>
		<rdfs:comment xml:lang="OWLManchester">platform:implementsInterface some JavaxAnnotationProcessingAPI</rdfs:comment>
	</owl:Class>
	<owl:Class rdf:about="&java-se-6;JavaxLangModelClassLibrary">
		<rdfs:subClassOf rdf:resource="&java;JavaClassLibrary"/>
		<rdfs:comment xml:lang="en">JavaLibrary implementing the javax.lang.model package for Java SE 6</rdfs:comment>
		<rdfs:comment xml:lang="OWLManchester">platform:implementsInterface some JavaxLangModelAPI</rdfs:comment>
	</owl:Class>
	<owl:Class rdf:about="&java-se-6;JavaxLangModelElementClassLibrary">
		<rdfs:subClassOf rdf:resource="&java;JavaClassLibrary"/>
		<rdfs:comment xml:lang="en">JavaLibrary implementing the javax.lang.model.element package for Java SE 6</rdfs:comment>
		<rdfs:comment xml:lang="OWLManchester">platform:implementsInterface some JavaxLangModelElementAPI</rdfs:comment>
	</owl:Class>
	<owl:Class rdf:about="&java-se-6;JavaxLangModelUtilClassLibrary">
		<rdfs:subClassOf rdf:resource="&java;JavaClassLibrary"/>
		<rdfs:comment xml:lang="en">JavaLibrary implementing the javax.lang.model.util package for Java SE 6</rdfs:comment>
		<rdfs:comment xml:lang="OWLManchester">platform:implementsInterface some JavaxLangModelUtilAPI</rdfs:comment>
	</owl:Class>
	<owl:Class rdf:about="&java-se-6;JavaxLangModelTypeClassLibrary">
		<rdfs:subClassOf rdf:resource="&java;JavaClassLibrary"/>
		<rdfs:comment xml:lang="en">JavaLibrary implementing the javax.lang.model.type package for Java SE 6</rdfs:comment>
		<rdfs:comment xml:lang="OWLManchester">platform:implementsInterface some JavaxLangModelTypeAPI</rdfs:comment>
	</owl:Class>
	<owl:Class rdf:about="&java-se-6;JavaxToolsClassLibrary">
		<rdfs:subClassOf rdf:resource="&java;JavaClassLibrary"/>
		<rdfs:comment xml:lang="en">JavaLibrary implementing the javax.tools package for Java SE 6</rdfs:comment>
		<rdfs:comment xml:lang="OWLManchester">platform:implementsInterface some JavaxToolsAPI</rdfs:comment>
	</owl:Class>
	<owl:Class rdf:about="&java-se-6;JavaxImageioClassLibrary">
		<rdfs:subClassOf rdf:resource="&j2se-5_0;JavaxImageioClassLibrary"/>
		<rdfs:comment xml:lang="en">JavaLibrary implementing the javax.imageio package for Java SE 6</rdfs:comment>
		<rdfs:comment xml:lang="OWLManchester">platform:implementsInterface some JavaxImageioAPI</rdfs:comment>
	</owl:Class>
	<owl:Class rdf:about="&java-se-6;JavaxImageioMetadataClassLibrary">
		<owl:equivalentClass rdf:resource="&j2se-5_0;JavaxImageioMetadataClassLibrary"/>
		<rdfs:subClassOf rdf:resource="&java;JavaClassLibrary"/>
		<rdfs:comment xml:lang="en">JavaLibrary implementing the javax.imageio.metadata package for Java SE 6</rdfs:comment>
		<rdfs:comment xml:lang="OWLManchester">platform:implementsInterface some JavaxImageioMetadataAPI</rdfs:comment>
	</owl:Class>
	<owl:Class rdf:about="&java-se-6;JavaxImageioStreamClassLibrary">
		<owl:equivalentClass rdf:resource="&j2se-5_0;JavaxImageioStreamClassLibrary"/>
		<rdfs:subClassOf rdf:resource="&java;JavaClassLibrary"/>
		<rdfs:comment xml:lang="en">JavaLibrary implementing the javax.imageio.stream package for Java SE 6</rdfs:comment>
		<rdfs:comment xml:lang="OWLManchester">platform:implementsInterface some JavaxImageioStreamAPI</rdfs:comment>
	</owl:Class>
	<owl:Class rdf:about="&java-se-6;JavaxImageioSpiClassLibrary">
		<owl:equivalentClass rdf:resource="&j2se-5_0;JavaxImageioSpiClassLibrary"/>
		<rdfs:subClassOf rdf:resource="&java;JavaClassLibrary"/>
		<rdfs:comment xml:lang="en">JavaLibrary implementing the javax.imageio.spi package for Java SE 6</rdfs:comment>
		<rdfs:comment xml:lang="OWLManchester">platform:implementsInterface some JavaxImageioSpiAPI</rdfs:comment>
	</owl:Class>
	<owl:Class rdf:about="&java-se-6;JavaxImageioEventClassLibrary">
		<owl:equivalentClass rdf:resource="&j2se-5_0;JavaxImageioEventClassLibrary"/>
		<rdfs:subClassOf rdf:resource="&java;JavaClassLibrary"/>
		<rdfs:comment xml:lang="en">JavaLibrary implementing the javax.imageio.event package for Java SE 6</rdfs:comment>
		<rdfs:comment xml:lang="OWLManchester">platform:implementsInterface some JavaxImageioEventAPI</rdfs:comment>
	</owl:Class>
	<owl:Class rdf:about="&java-se-6;JavaxImageioPluginsBmpClassLibrary">
		<owl:equivalentClass rdf:resource="&j2se-5_0;JavaxImageioPluginsBmpClassLibrary"/>
		<rdfs:subClassOf rdf:resource="&java;JavaClassLibrary"/>
		<rdfs:comment xml:lang="en">JavaLibrary implementing the javax.imageio.plugins.bmp package for Java SE 6</rdfs:comment>
		<rdfs:comment xml:lang="OWLManchester">platform:implementsInterface some JavaxImageioPluginsBmpAPI</rdfs:comment>
	</owl:Class>
	<owl:Class rdf:about="&java-se-6;JavaxImageioPluginsJpegClassLibrary">
		<owl:equivalentClass rdf:resource="&j2se-5_0;JavaxImageioPluginsJpegClassLibrary"/>
		<rdfs:subClassOf rdf:resource="&java;JavaClassLibrary"/>
		<rdfs:comment xml:lang="en">JavaLibrary implementing the javax.imageio.plugins.jpeg package for Java SE 6</rdfs:comment>
		<rdfs:comment xml:lang="OWLManchester">platform:implementsInterface some JavaxImageioPluginsJpegAPI</rdfs:comment>
	</owl:Class>
	<owl:Class rdf:about="&java-se-6;JavaxJwsClassLibrary">
		<rdfs:subClassOf rdf:resource="&java;JavaClassLibrary"/>
		<rdfs:comment xml:lang="en">JavaLibrary implementing the javax.jws package for Java SE 6</rdfs:comment>
		<rdfs:comment xml:lang="OWLManchester">platform:implementsInterface some JavaxJwsAPI</rdfs:comment>
	</owl:Class>
	<owl:Class rdf:about="&java-se-6;JavaxJwsSoapClassLibrary">
		<rdfs:subClassOf rdf:resource="&java;JavaClassLibrary"/>
		<rdfs:comment xml:lang="en">JavaLibrary implementing the javax.jws.soap package for Java SE 6</rdfs:comment>
		<rdfs:comment xml:lang="OWLManchester">platform:implementsInterface some JavaxJwsSoapAPI</rdfs:comment>
	</owl:Class>
	<owl:Class rdf:about="&java-se-6;JavaxRmiClassLibrary">
		<owl:equivalentClass rdf:resource="&j2se-5_0;JavaxRmiClassLibrary"/>
		<rdfs:subClassOf rdf:resource="&java;JavaClassLibrary"/>
		<rdfs:comment xml:lang="en">JavaLibrary implementing the javax.rmi package for Java SE 6</rdfs:comment>
		<rdfs:comment xml:lang="OWLManchester">platform:implementsInterface some JavaxRmiAPI</rdfs:comment>
	</owl:Class>
	<owl:Class rdf:about="&java-se-6;JavaxRmiCORBAClassLibrary">
		<owl:equivalentClass rdf:resource="&j2se-5_0;JavaxRmiCORBAClassLibrary"/>
		<rdfs:subClassOf rdf:resource="&java;JavaClassLibrary"/>
		<rdfs:comment xml:lang="en">JavaLibrary implementing the javax.rmi.CORBA package for Java SE 6</rdfs:comment>
		<rdfs:comment xml:lang="OWLManchester">platform:implementsInterface some JavaxRmiCORBAAPI</rdfs:comment>
	</owl:Class>
	<owl:Class rdf:about="&java-se-6;JavaxRmiSslClassLibrary">
		<owl:equivalentClass rdf:resource="&j2se-5_0;JavaxRmiSslClassLibrary"/>
		<rdfs:subClassOf rdf:resource="&java;JavaClassLibrary"/>
		<rdfs:comment xml:lang="en">JavaLibrary implementing the javax.rmi.ssl package for Java SE 6</rdfs:comment>
		<rdfs:comment xml:lang="OWLManchester">platform:implementsInterface some JavaxRmiSslAPI</rdfs:comment>
	</owl:Class>
	<owl:Class rdf:about="&java-se-6;JavaxNamingClassLibrary">
		<rdfs:subClassOf rdf:resource="&j2se-5_0;JavaxNamingClassLibrary"/>
		<rdfs:comment xml:lang="en">JavaLibrary implementing the javax.naming package for Java SE 6</rdfs:comment>
		<rdfs:comment xml:lang="OWLManchester">platform:implementsInterface some JavaxNamingAPI</rdfs:comment>
	</owl:Class>
	<owl:Class rdf:about="&java-se-6;JavaxNamingDirectoryClassLibrary">
		<rdfs:subClassOf rdf:resource="&j2se-5_0;JavaxNamingDirectoryClassLibrary"/>
		<rdfs:comment xml:lang="en">JavaLibrary implementing the javax.naming.directory package for Java SE 6</rdfs:comment>
		<rdfs:comment xml:lang="OWLManchester">platform:implementsInterface some JavaxNamingDirectoryAPI</rdfs:comment>
	</owl:Class>
	<owl:Class rdf:about="&java-se-6;JavaxNamingEventClassLibrary">
		<owl:equivalentClass rdf:resource="&j2se-5_0;JavaxNamingEventClassLibrary"/>
		<rdfs:subClassOf rdf:resource="&java;JavaClassLibrary"/>
		<rdfs:comment xml:lang="en">JavaLibrary implementing the javax.naming.event package for Java SE 6</rdfs:comment>
		<rdfs:comment xml:lang="OWLManchester">platform:implementsInterface some JavaxNamingEventAPI</rdfs:comment>
	</owl:Class>
	<owl:Class rdf:about="&java-se-6;JavaxNamingLdapClassLibrary">
		<rdfs:subClassOf rdf:resource="&j2se-5_0;JavaxNamingLdapClassLibrary"/>
		<rdfs:comment xml:lang="en">JavaLibrary implementing the javax.naming.ldap package for Java SE 6</rdfs:comment>
		<rdfs:comment xml:lang="OWLManchester">platform:implementsInterface some JavaxNamingLdapAPI</rdfs:comment>
	</owl:Class>
	<owl:Class rdf:about="&java-se-6;JavaxNamingSpiClassLibrary">
		<owl:equivalentClass rdf:resource="&j2se-5_0;JavaxNamingSpiClassLibrary"/>
		<rdfs:subClassOf rdf:resource="&java;JavaClassLibrary"/>
		<rdfs:comment xml:lang="en">JavaLibrary implementing the javax.naming.spi package for Java SE 6</rdfs:comment>
		<rdfs:comment xml:lang="OWLManchester">platform:implementsInterface some JavaxNamingSpiAPI</rdfs:comment>
	</owl:Class>
	<owl:Class rdf:about="&java-se-6;JavaxPrintClassLibrary">
		<owl:equivalentClass rdf:resource="&j2se-5_0;JavaxPrintClassLibrary"/>
		<rdfs:subClassOf rdf:resource="&java;JavaClassLibrary"/>
		<rdfs:comment xml:lang="en">JavaLibrary implementing the javax.print package for Java SE 6</rdfs:comment>
		<rdfs:comment xml:lang="OWLManchester">platform:implementsInterface some JavaxPrintAPI</rdfs:comment>
	</owl:Class>
	<owl:Class rdf:about="&java-se-6;JavaxPrintAttributeClassLibrary">
		<owl:equivalentClass rdf:resource="&j2se-5_0;JavaxPrintAttributeClassLibrary"/>
		<rdfs:subClassOf rdf:resource="&java;JavaClassLibrary"/>
		<rdfs:comment xml:lang="en">JavaLibrary implementing the javax.print.attribute package for Java SE 6</rdfs:comment>
		<rdfs:comment xml:lang="OWLManchester">platform:implementsInterface some JavaxPrintAttributeAPI</rdfs:comment>
	</owl:Class>
	<owl:Class rdf:about="&java-se-6;JavaxPrintAttributeStandardClassLibrary">
		<owl:equivalentClass rdf:resource="&j2se-5_0;JavaxPrintAttributeStandardClassLibrary"/>
		<rdfs:subClassOf rdf:resource="&java;JavaClassLibrary"/>
		<rdfs:comment xml:lang="en">JavaLibrary implementing the javax.print.attribute.standard package for Java SE 6</rdfs:comment>
		<rdfs:comment xml:lang="OWLManchester">platform:implementsInterface some JavaxPrintAttributeStandardAPI</rdfs:comment>
	</owl:Class>
	<owl:Class rdf:about="&java-se-6;JavaxPrintEventClassLibrary">
		<owl:equivalentClass rdf:resource="&j2se-5_0;JavaxPrintEventClassLibrary"/>
		<rdfs:subClassOf rdf:resource="&java;JavaClassLibrary"/>
		<rdfs:comment xml:lang="en">JavaLibrary implementing the javax.print.event package for Java SE 6</rdfs:comment>
		<rdfs:comment xml:lang="OWLManchester">platform:implementsInterface some JavaxPrintEventAPI</rdfs:comment>
	</owl:Class>
	<owl:Class rdf:about="&java-se-6;JavaxScriptClassLibrary">
		<rdfs:subClassOf rdf:resource="&java;JavaClassLibrary"/>
		<rdfs:comment xml:lang="en">JavaLibrary implementing the javax.script package for Java SE 6</rdfs:comment>
		<rdfs:comment xml:lang="OWLManchester">platform:implementsInterface some JavaxScriptAPI</rdfs:comment>
	</owl:Class>
	<owl:Class rdf:about="&java-se-6;JavaxSmartcardioClassLibrary">
		<rdfs:subClassOf rdf:resource="&java;JavaClassLibrary"/>
		<rdfs:comment xml:lang="en">JavaLibrary implementing the javax.smartcardio package for Java SE 6</rdfs:comment>
		<rdfs:comment xml:lang="OWLManchester">platform:implementsInterface some JavaxSmartcardioAPI</rdfs:comment>
	</owl:Class>
	<owl:Class rdf:about="&java-se-6;JavaxSoundMidiClassLibrary">
		<owl:equivalentClass rdf:resource="&j2se-5_0;JavaxSoundMidiClassLibrary"/>
		<rdfs:subClassOf rdf:resource="&java;JavaClassLibrary"/>
		<rdfs:comment xml:lang="en">JavaLibrary implementing the javax.sound.midi package for Java SE 6</rdfs:comment>
		<rdfs:comment xml:lang="OWLManchester">platform:implementsInterface some JavaxSoundMidiAPI</rdfs:comment>
	</owl:Class>
	<owl:Class rdf:about="&java-se-6;JavaxSoundMidiSpiClassLibrary">
		<owl:equivalentClass rdf:resource="&j2se-5_0;JavaxSoundMidiSpiClassLibrary"/>
		<rdfs:subClassOf rdf:resource="&java;JavaClassLibrary"/>
		<rdfs:comment xml:lang="en">JavaLibrary implementing the javax.sound.midi.spi package for Java SE 6</rdfs:comment>
		<rdfs:comment xml:lang="OWLManchester">platform:implementsInterface some JavaxSoundMidiSpiAPI</rdfs:comment>
	</owl:Class>
	<owl:Class rdf:about="&java-se-6;JavaxSoundSampledClassLibrary">
		<owl:equivalentClass rdf:resource="&j2se-5_0;JavaxSoundSampledClassLibrary"/>
		<rdfs:subClassOf rdf:resource="&java;JavaClassLibrary"/>
		<rdfs:comment xml:lang="en">JavaLibrary implementing the javax.sound.sampled package for Java SE 6</rdfs:comment>
		<rdfs:comment xml:lang="OWLManchester">platform:implementsInterface some JavaxSoundSampledAPI</rdfs:comment>
	</owl:Class>
	<owl:Class rdf:about="&java-se-6;JavaxSoundSampledSpiClassLibrary">
		<owl:equivalentClass rdf:resource="&j2se-5_0;JavaxSoundSampledSpiClassLibrary"/>
		<rdfs:subClassOf rdf:resource="&java;JavaClassLibrary"/>
		<rdfs:comment xml:lang="en">JavaLibrary implementing the javax.sound.sampled.spi package for Java SE 6</rdfs:comment>
		<rdfs:comment xml:lang="OWLManchester">platform:implementsInterface some JavaxSoundSampledSpiAPI</rdfs:comment>
	</owl:Class>
	<owl:Class rdf:about="&java-se-6;JavaxSqlClassLibrary">
		<rdfs:subClassOf rdf:resource="&j2se-5_0;JavaxSqlClassLibrary"/>
		<rdfs:comment xml:lang="en">JavaLibrary implementing the javax.sql package for Java SE 6</rdfs:comment>
		<rdfs:comment xml:lang="OWLManchester">platform:implementsInterface some JavaxSqlAPI</rdfs:comment>
	</owl:Class>
	<owl:Class rdf:about="&java-se-6;JavaxSqlRowsetClassLibrary">
		<rdfs:subClassOf rdf:resource="&j2se-5_0;JavaxSqlRowsetClassLibrary"/>
		<rdfs:comment xml:lang="en">JavaLibrary implementing the javax.sql.rowset package for Java SE 6</rdfs:comment>
		<rdfs:comment xml:lang="OWLManchester">platform:implementsInterface some JavaxSqlRowsetAPI</rdfs:comment>
	</owl:Class>
	<owl:Class rdf:about="&java-se-6;JavaxSqlRowsetSpiClassLibrary">
		<rdfs:subClassOf rdf:resource="&j2se-5_0;JavaxSqlRowsetSpiClassLibrary"/>
		<rdfs:comment xml:lang="en">JavaLibrary implementing the javax.sql.rowset.spi package for Java SE 6</rdfs:comment>
		<rdfs:comment xml:lang="OWLManchester">platform:implementsInterface some JavaxSqlRowsetSpiAPI</rdfs:comment>
	</owl:Class>
	<owl:Class rdf:about="&java-se-6;JavaxSqlRowsetSerialClassLibrary">
		<rdfs:subClassOf rdf:resource="&j2se-5_0;JavaxSqlRowsetSerialClassLibrary"/>
		<rdfs:comment xml:lang="en">JavaLibrary implementing the javax.sql.rowset.serial package for Java SE 6</rdfs:comment>
		<rdfs:comment xml:lang="OWLManchester">platform:implementsInterface some JavaxSqlRowsetSerialAPI</rdfs:comment>
	</owl:Class>
	<owl:Class rdf:about="&java-se-6;JavaxTransactionClassLibrary">
		<owl:equivalentClass rdf:resource="&j2se-5_0;JavaxTransactionClassLibrary"/>
		<rdfs:subClassOf rdf:resource="&java;JavaClassLibrary"/>
		<rdfs:comment xml:lang="en">JavaLibrary implementing the javax.transaction package for Java SE 6</rdfs:comment>
		<rdfs:comment xml:lang="OWLManchester">platform:implementsInterface some JavaxTransactionAPI</rdfs:comment>
	</owl:Class>
	<owl:Class rdf:about="&java-se-6;JavaxTransactionXaClassLibrary">
		<owl:equivalentClass rdf:resource="&j2se-5_0;JavaxTransactionXaClassLibrary"/>
		<rdfs:subClassOf rdf:resource="&java;JavaClassLibrary"/>
		<rdfs:comment xml:lang="en">JavaLibrary implementing the javax.transaction.xa package for Java SE 6</rdfs:comment>
		<rdfs:comment xml:lang="OWLManchester">platform:implementsInterface some JavaxTransactionXaAPI</rdfs:comment>
	</owl:Class>
	<owl:Class rdf:about="&java-se-6;JavaLangClassLibrary">
		<rdfs:subClassOf rdf:resource="&j2se-5_0;JavaLangClassLibrary"/>
		<rdfs:comment xml:lang="en">JavaLibrary implementing the java.lang package for Java SE 6</rdfs:comment>
		<rdfs:comment xml:lang="OWLManchester">platform:implementsInterface some JavaLangAPI</rdfs:comment>
	</owl:Class>
	<owl:Class rdf:about="&java-se-6;JavaLangAnnotationClassLibrary">
		<rdfs:subClassOf rdf:resource="&j2se-5_0;JavaLangAnnotationClassLibrary"/>
		<rdfs:comment xml:lang="en">JavaLibrary implementing the java.lang.annotation package for Java SE 6</rdfs:comment>
		<rdfs:comment xml:lang="OWLManchester">platform:implementsInterface some JavaLangAnnotationAPI</rdfs:comment>
	</owl:Class>
	<owl:Class rdf:about="&java-se-6;JavaLangReflectClassLibrary">
		<owl:equivalentClass rdf:resource="&j2se-5_0;JavaLangReflectClassLibrary"/>
		<rdfs:subClassOf rdf:resource="&java;JavaClassLibrary"/>
		<rdfs:comment xml:lang="en">JavaLibrary implementing the java.lang.reflect package for Java SE 6</rdfs:comment>
		<rdfs:comment xml:lang="OWLManchester">platform:implementsInterface some JavaLangReflectAPI</rdfs:comment>
	</owl:Class>
	<owl:Class rdf:about="&java-se-6;JavaLangInstrumentClassLibrary">
		<rdfs:subClassOf rdf:resource="&j2se-5_0;JavaLangInstrumentClassLibrary"/>
		<rdfs:comment xml:lang="en">JavaLibrary implementing the java.lang.instrument package for Java SE 6</rdfs:comment>
		<rdfs:comment xml:lang="OWLManchester">platform:implementsInterface some JavaLangInstrumentAPI</rdfs:comment>
	</owl:Class>
	<owl:Class rdf:about="&java-se-6;JavaLangManagementClassLibrary">
		<rdfs:subClassOf rdf:resource="&j2se-5_0;JavaLangManagementClassLibrary"/>
		<rdfs:comment xml:lang="en">JavaLibrary implementing the java.lang.management package for Java SE 6</rdfs:comment>
		<rdfs:comment xml:lang="OWLManchester">platform:implementsInterface some JavaLangManagementAPI</rdfs:comment>
	</owl:Class>
	<owl:Class rdf:about="&java-se-6;JavaLangRefClassLibrary">
		<owl:equivalentClass rdf:resource="&j2se-5_0;JavaLangRefClassLibrary"/>
		<rdfs:subClassOf rdf:resource="&java;JavaClassLibrary"/>
		<rdfs:comment xml:lang="en">JavaLibrary implementing the java.lang.ref package for Java SE 6</rdfs:comment>
		<rdfs:comment xml:lang="OWLManchester">platform:implementsInterface some JavaLangRefAPI</rdfs:comment>
	</owl:Class>
	<owl:Class rdf:about="&java-se-6;JavaAwtClassLibrary">
		<rdfs:subClassOf rdf:resource="&j2se-5_0;JavaAwtClassLibrary"/>
		<rdfs:comment xml:lang="en">JavaLibrary implementing the java.awt package for Java SE 6</rdfs:comment>
		<rdfs:comment xml:lang="OWLManchester">platform:implementsInterface some JavaAwtAPI</rdfs:comment>
	</owl:Class>
	<owl:Class rdf:about="&java-se-6;JavaAwtPrintClassLibrary">
		<rdfs:subClassOf rdf:resource="&j2se-5_0;JavaAwtPrintClassLibrary"/>
		<rdfs:comment xml:lang="en">JavaLibrary implementing the java.awt.print package for Java SE 6</rdfs:comment>
		<rdfs:comment xml:lang="OWLManchester">platform:implementsInterface some JavaAwtPrintAPI</rdfs:comment>
	</owl:Class>
	<owl:Class rdf:about="&java-se-6;JavaAwtDatatransferClassLibrary">
		<owl:equivalentClass rdf:resource="&j2se-5_0;JavaAwtDatatransferClassLibrary"/>
		<rdfs:subClassOf rdf:resource="&java;JavaClassLibrary"/>
		<rdfs:comment xml:lang="en">JavaLibrary implementing the java.awt.datatransfer package for Java SE 6</rdfs:comment>
		<rdfs:comment xml:lang="OWLManchester">platform:implementsInterface some JavaAwtDatatransferAPI</rdfs:comment>
	</owl:Class>
	<owl:Class rdf:about="&java-se-6;JavaAwtEventClassLibrary">
		<rdfs:subClassOf rdf:resource="&j2se-5_0;JavaAwtEventClassLibrary"/>
		<rdfs:comment xml:lang="en">JavaLibrary implementing the java.awt.event package for Java SE 6</rdfs:comment>
		<rdfs:comment xml:lang="OWLManchester">platform:implementsInterface some JavaAwtEventAPI</rdfs:comment>
	</owl:Class>
	<owl:Class rdf:about="&java-se-6;JavaAwtImageClassLibrary">
		<rdfs:subClassOf rdf:resource="&j2se-5_0;JavaAwtImageClassLibrary"/>
		<rdfs:comment xml:lang="en">JavaLibrary implementing the java.awt.image package for Java SE 6</rdfs:comment>
		<rdfs:comment xml:lang="OWLManchester">platform:implementsInterface some JavaAwtImageAPI</rdfs:comment>
	</owl:Class>
	<owl:Class rdf:about="&java-se-6;JavaAwtImageRenderableClassLibrary">
		<owl:equivalentClass rdf:resource="&j2se-5_0;JavaAwtImageRenderableClassLibrary"/>
		<rdfs:subClassOf rdf:resource="&java;JavaClassLibrary"/>
		<rdfs:comment xml:lang="en">JavaLibrary implementing the java.awt.image.renderable package for Java SE 6</rdfs:comment>
		<rdfs:comment xml:lang="OWLManchester">platform:implementsInterface some JavaAwtImageRenderableAPI</rdfs:comment>
	</owl:Class>
	<owl:Class rdf:about="&java-se-6;JavaAwtGeomClassLibrary">
		<rdfs:subClassOf rdf:resource="&java;JavaClassLibrary"/>
		<rdfs:comment xml:lang="en">JavaLibrary implementing the java.awt.geom package for Java SE 6</rdfs:comment>
		<rdfs:comment xml:lang="OWLManchester">platform:implementsInterface some JavaAwtGeomAPI</rdfs:comment>
	</owl:Class>
	<owl:Class rdf:about="&java-se-6;JavaAwtImClassLibrary">
		<owl:equivalentClass rdf:resource="&j2se-5_0;JavaAwtImClassLibrary"/>
		<rdfs:subClassOf rdf:resource="&java;JavaClassLibrary"/>
		<rdfs:comment xml:lang="en">JavaLibrary implementing the java.awt.im package for Java SE 6</rdfs:comment>
		<rdfs:comment xml:lang="OWLManchester">platform:implementsInterface some JavaAwtImAPI</rdfs:comment>
	</owl:Class>
	<owl:Class rdf:about="&java-se-6;JavaAwtImSpiClassLibrary">
		<owl:equivalentClass rdf:resource="&j2se-5_0;JavaAwtImSpiClassLibrary"/>
		<rdfs:subClassOf rdf:resource="&java;JavaClassLibrary"/>
		<rdfs:comment xml:lang="en">JavaLibrary implementing the java.awt.im.spi package for Java SE 6</rdfs:comment>
		<rdfs:comment xml:lang="OWLManchester">platform:implementsInterface some JavaAwtImSpiAPI</rdfs:comment>
	</owl:Class>
	<owl:Class rdf:about="&java-se-6;JavaAwtColorClassLibrary">
		<owl:equivalentClass rdf:resource="&j2se-5_0;JavaAwtColorClassLibrary"/>
		<rdfs:subClassOf rdf:resource="&java;JavaClassLibrary"/>
		<rdfs:comment xml:lang="en">JavaLibrary implementing the java.awt.color package for Java SE 6</rdfs:comment>
		<rdfs:comment xml:lang="OWLManchester">platform:implementsInterface some JavaAwtColorAPI</rdfs:comment>
	</owl:Class>
	<owl:Class rdf:about="&java-se-6;JavaAwtDndClassLibrary">
		<owl:equivalentClass rdf:resource="&j2se-5_0;JavaAwtDndClassLibrary"/>
		<rdfs:subClassOf rdf:resource="&java;JavaClassLibrary"/>
		<rdfs:comment xml:lang="en">JavaLibrary implementing the java.awt.dnd package for Java SE 6</rdfs:comment>
		<rdfs:comment xml:lang="OWLManchester">platform:implementsInterface some JavaAwtDndAPI</rdfs:comment>
	</owl:Class>
	<owl:Class rdf:about="&java-se-6;JavaAwtFontClassLibrary">
		<rdfs:subClassOf rdf:resource="&j2se-5_0;JavaAwtFontClassLibrary"/>
		<rdfs:comment xml:lang="en">JavaLibrary implementing the java.awt.font package for Java SE 6</rdfs:comment>
		<rdfs:comment xml:lang="OWLManchester">platform:implementsInterface some JavaAwtFontAPI</rdfs:comment>
	</owl:Class>
	<owl:Class rdf:about="&java-se-6;JavaNetClassLibrary">
		<rdfs:subClassOf rdf:resource="&j2se-5_0;JavaNetClassLibrary"/>
		<rdfs:comment xml:lang="en">JavaLibrary implementing the java.net package for Java SE 6</rdfs:comment>
		<rdfs:comment xml:lang="OWLManchester">platform:implementsInterface some JavaNetAPI</rdfs:comment>
	</owl:Class>
	<owl:Class rdf:about="&java-se-6;JavaIoClassLibrary">
		<rdfs:subClassOf rdf:resource="&j2se-5_0;JavaIoClassLibrary"/>
		<rdfs:comment xml:lang="en">JavaLibrary implementing the java.io package for Java SE 6</rdfs:comment>
		<rdfs:comment xml:lang="OWLManchester">platform:implementsInterface some JavaIoAPI</rdfs:comment>
	</owl:Class>
	<owl:Class rdf:about="&java-se-6;JavaSecurityClassLibrary">
		<rdfs:subClassOf rdf:resource="&j2se-5_0;JavaSecurityClassLibrary"/>
		<rdfs:comment xml:lang="en">JavaLibrary implementing the java.security package for Java SE 6</rdfs:comment>
		<rdfs:comment xml:lang="OWLManchester">platform:implementsInterface some JavaSecurityAPI</rdfs:comment>
	</owl:Class>
	<owl:Class rdf:about="&java-se-6;JavaSecuritySpecClassLibrary">
		<owl:equivalentClass rdf:resource="&j2se-5_0;JavaSecuritySpecClassLibrary"/>
		<rdfs:subClassOf rdf:resource="&java;JavaClassLibrary"/>
		<rdfs:comment xml:lang="en">JavaLibrary implementing the java.security.spec package for Java SE 6</rdfs:comment>
		<rdfs:comment xml:lang="OWLManchester">platform:implementsInterface some JavaSecuritySpecAPI</rdfs:comment>
	</owl:Class>
	<owl:Class rdf:about="&java-se-6;JavaSecurityCertClassLibrary">
		<owl:equivalentClass rdf:resource="&j2se-5_0;JavaSecurityCertClassLibrary"/>
		<rdfs:subClassOf rdf:resource="&java;JavaClassLibrary"/>
		<rdfs:comment xml:lang="en">JavaLibrary implementing the java.security.cert package for Java SE 6</rdfs:comment>
		<rdfs:comment xml:lang="OWLManchester">platform:implementsInterface some JavaSecurityCertAPI</rdfs:comment>
	</owl:Class>
	<owl:Class rdf:about="&java-se-6;JavaSecurityAclClassLibrary">
		<owl:equivalentClass rdf:resource="&j2se-5_0;JavaSecurityAclClassLibrary"/>
		<rdfs:subClassOf rdf:resource="&java;JavaClassLibrary"/>
		<rdfs:comment xml:lang="en">JavaLibrary implementing the java.security.acl package for Java SE 6</rdfs:comment>
		<rdfs:comment xml:lang="OWLManchester">platform:implementsInterface some JavaSecurityAclAPI</rdfs:comment>
	</owl:Class>
	<owl:Class rdf:about="&java-se-6;JavaSecurityInterfacesClassLibrary">
		<owl:equivalentClass rdf:resource="&j2se-5_0;JavaSecurityInterfacesClassLibrary"/>
		<rdfs:subClassOf rdf:resource="&java;JavaClassLibrary"/>
		<rdfs:comment xml:lang="en">JavaLibrary implementing the java.security.interfaces package for Java SE 6</rdfs:comment>
		<rdfs:comment xml:lang="OWLManchester">platform:implementsInterface some JavaSecurityInterfacesAPI</rdfs:comment>
	</owl:Class>
	<owl:Class rdf:about="&java-se-6;JavaMathClassLibrary">
		<rdfs:subClassOf rdf:resource="&j2se-5_0;JavaMathClassLibrary"/>
		<rdfs:comment xml:lang="en">JavaLibrary implementing the java.math package for Java SE 6</rdfs:comment>
		<rdfs:comment xml:lang="OWLManchester">platform:implementsInterface some JavaMathAPI</rdfs:comment>
	</owl:Class>
	<owl:Class rdf:about="&java-se-6;JavaNioClassLibrary">
		<rdfs:subClassOf rdf:resource="&j2se-5_0;JavaNioClassLibrary"/>
		<rdfs:comment xml:lang="en">JavaLibrary implementing the java.nio package for Java SE 6</rdfs:comment>
		<rdfs:comment xml:lang="OWLManchester">platform:implementsInterface some JavaNioAPI</rdfs:comment>
	</owl:Class>
	<owl:Class rdf:about="&java-se-6;JavaNioChannelsClassLibrary">
		<owl:equivalentClass rdf:resource="&j2se-5_0;JavaNioChannelsClassLibrary"/>
		<rdfs:subClassOf rdf:resource="&java;JavaClassLibrary"/>
		<rdfs:comment xml:lang="en">JavaLibrary implementing the java.nio.channels package for Java SE 6</rdfs:comment>
		<rdfs:comment xml:lang="OWLManchester">platform:implementsInterface some JavaNioChannelsAPI</rdfs:comment>
	</owl:Class>
	<owl:Class rdf:about="&java-se-6;JavaNioChannelsSpiClassLibrary">
		<owl:equivalentClass rdf:resource="&j2se-5_0;JavaNioChannelsSpiClassLibrary"/>
		<rdfs:subClassOf rdf:resource="&java;JavaClassLibrary"/>
		<rdfs:comment xml:lang="en">JavaLibrary implementing the java.nio.channels.spi package for Java SE 6</rdfs:comment>
		<rdfs:comment xml:lang="OWLManchester">platform:implementsInterface some JavaNioChannelsSpiAPI</rdfs:comment>
	</owl:Class>
	<owl:Class rdf:about="&java-se-6;JavaNioCharsetClassLibrary">
		<owl:equivalentClass rdf:resource="&j2se-5_0;JavaNioCharsetClassLibrary"/>
		<rdfs:subClassOf rdf:resource="&java;JavaClassLibrary"/>
		<rdfs:comment xml:lang="en">JavaLibrary implementing the java.nio.charset package for Java SE 6</rdfs:comment>
		<rdfs:comment xml:lang="OWLManchester">platform:implementsInterface some JavaNioCharsetAPI</rdfs:comment>
	</owl:Class>
	<owl:Class rdf:about="&java-se-6;JavaNioCharsetSpiClassLibrary">
		<owl:equivalentClass rdf:resource="&j2se-5_0;JavaNioCharsetSpiClassLibrary"/>
		<rdfs:subClassOf rdf:resource="&java;JavaClassLibrary"/>
		<rdfs:comment xml:lang="en">JavaLibrary implementing the java.nio.charset.spi package for Java SE 6</rdfs:comment>
		<rdfs:comment xml:lang="OWLManchester">platform:implementsInterface some JavaNioCharsetSpiAPI</rdfs:comment>
	</owl:Class>
	<owl:Class rdf:about="&java-se-6;JavaUtilClassLibrary">
		<rdfs:subClassOf rdf:resource="&j2se-5_0;JavaUtilClassLibrary"/>
		<rdfs:comment xml:lang="en">JavaLibrary implementing the java.util package for Java SE 6</rdfs:comment>
		<rdfs:comment xml:lang="OWLManchester">platform:implementsInterface some JavaUtilAPI</rdfs:comment>
	</owl:Class>
	<owl:Class rdf:about="&java-se-6;JavaUtilJarClassLibrary">
		<owl:equivalentClass rdf:resource="&j2se-5_0;JavaUtilJarClassLibrary"/>
		<rdfs:subClassOf rdf:resource="&java;JavaClassLibrary"/>
		<rdfs:comment xml:lang="en">JavaLibrary implementing the java.util.jar package for Java SE 6</rdfs:comment>
		<rdfs:comment xml:lang="OWLManchester">platform:implementsInterface some JavaUtilJarAPI</rdfs:comment>
	</owl:Class>
	<owl:Class rdf:about="&java-se-6;JavaUtilSpiClassLibrary">
		<rdfs:subClassOf rdf:resource="&java;JavaClassLibrary"/>
		<rdfs:comment xml:lang="en">JavaLibrary implementing the java.util.spi package for Java SE 6</rdfs:comment>
		<rdfs:comment xml:lang="OWLManchester">platform:implementsInterface some JavaUtilSpiAPI</rdfs:comment>
	</owl:Class>
	<owl:Class rdf:about="&java-se-6;JavaUtilConcurrentClassLibrary">
		<rdfs:subClassOf rdf:resource="&java;JavaClassLibrary"/>
		<rdfs:comment xml:lang="en">JavaLibrary implementing the java.util.concurrent package for Java SE 6</rdfs:comment>
		<rdfs:comment xml:lang="OWLManchester">platform:implementsInterface some JavaUtilConcurrentAPI</rdfs:comment>
	</owl:Class>
	<owl:Class rdf:about="&java-se-6;JavaUtilConcurrentAtomicClassLibrary">
		<rdfs:subClassOf rdf:resource="&j2se-5_0;JavaUtilConcurrentAtomicClassLibrary"/>
		<rdfs:comment xml:lang="en">JavaLibrary implementing the java.util.concurrent.atomic package for Java SE 6</rdfs:comment>
		<rdfs:comment xml:lang="OWLManchester">platform:implementsInterface some JavaUtilConcurrentAtomicAPI</rdfs:comment>
	</owl:Class>
	<owl:Class rdf:about="&java-se-6;JavaUtilConcurrentLocksClassLibrary">
		<rdfs:subClassOf rdf:resource="&j2se-5_0;JavaUtilConcurrentLocksClassLibrary"/>
		<rdfs:comment xml:lang="en">JavaLibrary implementing the java.util.concurrent.locks package for Java SE 6</rdfs:comment>
		<rdfs:comment xml:lang="OWLManchester">platform:implementsInterface some JavaUtilConcurrentLocksAPI</rdfs:comment>
	</owl:Class>
	<owl:Class rdf:about="&java-se-6;JavaUtilZipClassLibrary">
		<rdfs:subClassOf rdf:resource="&j2se-5_0;JavaUtilZipClassLibrary"/>
		<rdfs:comment xml:lang="en">JavaLibrary implementing the java.util.zip package for Java SE 6</rdfs:comment>
		<rdfs:comment xml:lang="OWLManchester">platform:implementsInterface some JavaUtilZipAPI</rdfs:comment>
	</owl:Class>
	<owl:Class rdf:about="&java-se-6;JavaUtilLoggingClassLibrary">
		<rdfs:subClassOf rdf:resource="&j2se-5_0;JavaUtilLoggingClassLibrary"/>
		<rdfs:comment xml:lang="en">JavaLibrary implementing the java.util.logging package for Java SE 6</rdfs:comment>
		<rdfs:comment xml:lang="OWLManchester">platform:implementsInterface some JavaUtilLoggingAPI</rdfs:comment>
	</owl:Class>
	<owl:Class rdf:about="&java-se-6;JavaUtilPrefsClassLibrary">
		<owl:equivalentClass rdf:resource="&j2se-5_0;JavaUtilPrefsClassLibrary"/>
		<rdfs:subClassOf rdf:resource="&java;JavaClassLibrary"/>
		<rdfs:comment xml:lang="en">JavaLibrary implementing the java.util.prefs package for Java SE 6</rdfs:comment>
		<rdfs:comment xml:lang="OWLManchester">platform:implementsInterface some JavaUtilPrefsAPI</rdfs:comment>
	</owl:Class>
	<owl:Class rdf:about="&java-se-6;JavaUtilRegexClassLibrary">
		<owl:equivalentClass rdf:resource="&j2se-5_0;JavaUtilRegexClassLibrary"/>
		<rdfs:subClassOf rdf:resource="&java;JavaClassLibrary"/>
		<rdfs:comment xml:lang="en">JavaLibrary implementing the java.util.regex package for Java SE 6</rdfs:comment>
		<rdfs:comment xml:lang="OWLManchester">platform:implementsInterface some JavaUtilRegexAPI</rdfs:comment>
	</owl:Class>
	<owl:Class rdf:about="&java-se-6;JavaAppletClassLibrary">
		<rdfs:subClassOf rdf:resource="&j2se-5_0;JavaAppletClassLibrary"/>
		<rdfs:comment xml:lang="en">JavaLibrary implementing the java.applet package for Java SE 6</rdfs:comment>
		<rdfs:comment xml:lang="OWLManchester">platform:implementsInterface some JavaAppletAPI</rdfs:comment>
	</owl:Class>
	<owl:Class rdf:about="&java-se-6;JavaBeansClassLibrary">
		<rdfs:subClassOf rdf:resource="&j2se-5_0;JavaBeansClassLibrary"/>
		<rdfs:comment xml:lang="en">JavaLibrary implementing the java.beans package for Java SE 6</rdfs:comment>
		<rdfs:comment xml:lang="OWLManchester">platform:implementsInterface some JavaBeansAPI</rdfs:comment>
	</owl:Class>
	<owl:Class rdf:about="&java-se-6;JavaBeansBeancontextClassLibrary">
		<owl:equivalentClass rdf:resource="&j2se-5_0;JavaBeansBeancontextClassLibrary"/>
		<rdfs:subClassOf rdf:resource="&java;JavaClassLibrary"/>
		<rdfs:comment xml:lang="en">JavaLibrary implementing the java.beans.beancontext package for Java SE 6</rdfs:comment>
		<rdfs:comment xml:lang="OWLManchester">platform:implementsInterface some JavaBeansBeancontextAPI</rdfs:comment>
	</owl:Class>
	<owl:Class rdf:about="&java-se-6;JavaTextClassLibrary">
		<rdfs:subClassOf rdf:resource="&java;JavaClassLibrary"/>
		<rdfs:comment xml:lang="en">JavaLibrary implementing the java.text package for Java SE 6</rdfs:comment>
		<rdfs:comment xml:lang="OWLManchester">platform:implementsInterface some JavaTextAPI</rdfs:comment>
	</owl:Class>
	<owl:Class rdf:about="&java-se-6;JavaTextSpiClassLibrary">
		<rdfs:subClassOf rdf:resource="&java;JavaClassLibrary"/>
		<rdfs:comment xml:lang="en">JavaLibrary implementing the java.text.spi package for Java SE 6</rdfs:comment>
		<rdfs:comment xml:lang="OWLManchester">platform:implementsInterface some JavaTextSpiAPI</rdfs:comment>
	</owl:Class>
	<owl:Class rdf:about="&java-se-6;JavaRmiClassLibrary">
		<owl:equivalentClass rdf:resource="&j2se-5_0;JavaRmiClassLibrary"/>
		<rdfs:subClassOf rdf:resource="&java;JavaClassLibrary"/>
		<rdfs:comment xml:lang="en">JavaLibrary implementing the java.rmi package for Java SE 6</rdfs:comment>
		<rdfs:comment xml:lang="OWLManchester">platform:implementsInterface some JavaRmiAPI</rdfs:comment>
	</owl:Class>
	<owl:Class rdf:about="&java-se-6;JavaRmiActivationClassLibrary">
		<owl:equivalentClass rdf:resource="&j2se-5_0;JavaRmiActivationClassLibrary"/>
		<rdfs:subClassOf rdf:resource="&java;JavaClassLibrary"/>
		<rdfs:comment xml:lang="en">JavaLibrary implementing the java.rmi.activation package for Java SE 6</rdfs:comment>
		<rdfs:comment xml:lang="OWLManchester">platform:implementsInterface some JavaRmiActivationAPI</rdfs:comment>
	</owl:Class>
	<owl:Class rdf:about="&java-se-6;JavaRmiServerClassLibrary">
		<rdfs:subClassOf rdf:resource="&j2se-5_0;JavaRmiServerClassLibrary"/>
		<rdfs:comment xml:lang="en">JavaLibrary implementing the java.rmi.server package for Java SE 6</rdfs:comment>
		<rdfs:comment xml:lang="OWLManchester">platform:implementsInterface some JavaRmiServerAPI</rdfs:comment>
	</owl:Class>
	<owl:Class rdf:about="&java-se-6;JavaRmiDgcClassLibrary">
		<owl:equivalentClass rdf:resource="&j2se-5_0;JavaRmiDgcClassLibrary"/>
		<rdfs:subClassOf rdf:resource="&java;JavaClassLibrary"/>
		<rdfs:comment xml:lang="en">JavaLibrary implementing the java.rmi.dgc package for Java SE 6</rdfs:comment>
		<rdfs:comment xml:lang="OWLManchester">platform:implementsInterface some JavaRmiDgcAPI</rdfs:comment>
	</owl:Class>
	<owl:Class rdf:about="&java-se-6;JavaRmiRegistryClassLibrary">
		<owl:equivalentClass rdf:resource="&j2se-5_0;JavaRmiRegistryClassLibrary"/>
		<rdfs:subClassOf rdf:resource="&java;JavaClassLibrary"/>
		<rdfs:comment xml:lang="en">JavaLibrary implementing the java.rmi.registry package for Java SE 6</rdfs:comment>
		<rdfs:comment xml:lang="OWLManchester">platform:implementsInterface some JavaRmiRegistryAPI</rdfs:comment>
	</owl:Class>
	<owl:Class rdf:about="&java-se-6;JavaSqlClassLibrary">
		<rdfs:subClassOf rdf:resource="&j2se-5_0;JavaSqlClassLibrary"/>
		<rdfs:comment xml:lang="en">JavaLibrary implementing the java.sql package for Java SE 6</rdfs:comment>
		<rdfs:comment xml:lang="OWLManchester">platform:implementsInterface some JavaSqlAPI</rdfs:comment>
	</owl:Class>
	<owl:Class rdf:about="&java-se-6;OrgW3cDomClassLibrary">
		<owl:equivalentClass rdf:resource="&j2se-5_0;OrgW3cDomClassLibrary"/>
		<rdfs:subClassOf rdf:resource="&java;JavaClassLibrary"/>
		<rdfs:comment xml:lang="en">JavaLibrary implementing the org.w3c.dom package for Java SE 6</rdfs:comment>
		<rdfs:comment xml:lang="OWLManchester">platform:implementsInterface some OrgW3cDomAPI</rdfs:comment>
	</owl:Class>
	<owl:Class rdf:about="&java-se-6;OrgW3cDomLsClassLibrary">
		<owl:equivalentClass rdf:resource="&j2se-5_0;OrgW3cDomLsClassLibrary"/>
		<rdfs:subClassOf rdf:resource="&java;JavaClassLibrary"/>
		<rdfs:comment xml:lang="en">JavaLibrary implementing the org.w3c.dom.ls package for Java SE 6</rdfs:comment>
		<rdfs:comment xml:lang="OWLManchester">platform:implementsInterface some OrgW3cDomLsAPI</rdfs:comment>
	</owl:Class>
	<owl:Class rdf:about="&java-se-6;OrgW3cDomBootstrapClassLibrary">
		<owl:equivalentClass rdf:resource="&j2se-5_0;OrgW3cDomBootstrapClassLibrary"/>
		<rdfs:subClassOf rdf:resource="&java;JavaClassLibrary"/>
		<rdfs:comment xml:lang="en">JavaLibrary implementing the org.w3c.dom.bootstrap package for Java SE 6</rdfs:comment>
		<rdfs:comment xml:lang="OWLManchester">platform:implementsInterface some OrgW3cDomBootstrapAPI</rdfs:comment>
	</owl:Class>
	<owl:Class rdf:about="&java-se-6;OrgW3cDomCssClassLibrary">
		<owl:equivalentClass rdf:resource="&j2se-5_0;OrgW3cDomCssClassLibrary"/>
		<rdfs:subClassOf rdf:resource="&java;JavaClassLibrary"/>
		<rdfs:comment xml:lang="en">JavaLibrary implementing the org.w3c.dom.css package for Java SE 6</rdfs:comment>
		<rdfs:comment xml:lang="OWLManchester">platform:implementsInterface some OrgW3cDomCssAPI</rdfs:comment>
	</owl:Class>
	<owl:Class rdf:about="&java-se-6;OrgW3cDomStylesheetsClassLibrary">
		<owl:equivalentClass rdf:resource="&j2se-5_0;OrgW3cDomStylesheetsClassLibrary"/>
		<rdfs:subClassOf rdf:resource="&java;JavaClassLibrary"/>
		<rdfs:comment xml:lang="en">JavaLibrary implementing the org.w3c.dom.stylesheets package for Java SE 6</rdfs:comment>
		<rdfs:comment xml:lang="OWLManchester">platform:implementsInterface some OrgW3cDomStylesheetsAPI</rdfs:comment>
	</owl:Class>
	<owl:Class rdf:about="&java-se-6;OrgW3cDomViewsClassLibrary">
		<owl:equivalentClass rdf:resource="&j2se-5_0;OrgW3cDomViewsClassLibrary"/>
		<rdfs:subClassOf rdf:resource="&java;JavaClassLibrary"/>
		<rdfs:comment xml:lang="en">JavaLibrary implementing the org.w3c.dom.views package for Java SE 6</rdfs:comment>
		<rdfs:comment xml:lang="OWLManchester">platform:implementsInterface some OrgW3cDomViewsAPI</rdfs:comment>
	</owl:Class>
	<owl:Class rdf:about="&java-se-6;OrgW3cDomEventsClassLibrary">
		<owl:equivalentClass rdf:resource="&j2se-5_0;OrgW3cDomEventsClassLibrary"/>
		<rdfs:subClassOf rdf:resource="&java;JavaClassLibrary"/>
		<rdfs:comment xml:lang="en">JavaLibrary implementing the org.w3c.dom.events package for Java SE 6</rdfs:comment>
		<rdfs:comment xml:lang="OWLManchester">platform:implementsInterface some OrgW3cDomEventsAPI</rdfs:comment>
	</owl:Class>
	<owl:Class rdf:about="&java-se-6;OrgW3cDomHtmlClassLibrary">
		<owl:equivalentClass rdf:resource="&j2se-5_0;OrgW3cDomHtmlClassLibrary"/>
		<rdfs:subClassOf rdf:resource="&java;JavaClassLibrary"/>
		<rdfs:comment xml:lang="en">JavaLibrary implementing the org.w3c.dom.html package for Java SE 6</rdfs:comment>
		<rdfs:comment xml:lang="OWLManchester">platform:implementsInterface some OrgW3cDomHtmlAPI</rdfs:comment>
	</owl:Class>
	<owl:Class rdf:about="&java-se-6;OrgW3cDomTraversalClassLibrary">
		<owl:equivalentClass rdf:resource="&j2se-5_0;OrgW3cDomTraversalClassLibrary"/>
		<rdfs:subClassOf rdf:resource="&java;JavaClassLibrary"/>
		<rdfs:comment xml:lang="en">JavaLibrary implementing the org.w3c.dom.traversal package for Java SE 6</rdfs:comment>
		<rdfs:comment xml:lang="OWLManchester">platform:implementsInterface some OrgW3cDomTraversalAPI</rdfs:comment>
	</owl:Class>
	<owl:Class rdf:about="&java-se-6;OrgW3cDomRangesClassLibrary">
		<owl:equivalentClass rdf:resource="&j2se-5_0;OrgW3cDomRangesClassLibrary"/>
		<rdfs:subClassOf rdf:resource="&java;JavaClassLibrary"/>
		<rdfs:comment xml:lang="en">JavaLibrary implementing the org.w3c.dom.ranges package for Java SE 6</rdfs:comment>
		<rdfs:comment xml:lang="OWLManchester">platform:implementsInterface some OrgW3cDomRangesAPI</rdfs:comment>
	</owl:Class>
	<owl:Class rdf:about="&java-se-6;OrgW3cDomXpathClassLibrary">
		<rdfs:subClassOf rdf:resource="&java;JavaClassLibrary"/>
		<rdfs:comment xml:lang="en">JavaLibrary implementing the org.w3c.dom.xpath package for Java SE 6</rdfs:comment>
		<rdfs:comment xml:lang="OWLManchester">platform:implementsInterface some OrgW3cDomXpathAPI</rdfs:comment>
	</owl:Class>
	<owl:Class rdf:about="&java-se-6;OrgOmgCORBA_2_3ClassLibrary">
		<owl:equivalentClass rdf:resource="&j2se-5_0;OrgOmgCORBA_2_3ClassLibrary"/>
		<rdfs:subClassOf rdf:resource="&java;JavaClassLibrary"/>
		<rdfs:comment xml:lang="en">JavaLibrary implementing the org.omg.CORBA_2_3 package for Java SE 6</rdfs:comment>
		<rdfs:comment xml:lang="OWLManchester">platform:implementsInterface some OrgOmgCORBA_2_3API</rdfs:comment>
	</owl:Class>
	<owl:Class rdf:about="&java-se-6;OrgOmgCORBA_2_3PortableClassLibrary">
		<owl:equivalentClass rdf:resource="&j2se-5_0;OrgOmgCORBA_2_3PortableClassLibrary"/>
		<rdfs:subClassOf rdf:resource="&java;JavaClassLibrary"/>
		<rdfs:comment xml:lang="en">JavaLibrary implementing the org.omg.CORBA_2_3.portable package for Java SE 6</rdfs:comment>
		<rdfs:comment xml:lang="OWLManchester">platform:implementsInterface some OrgOmgCORBA_2_3PortableAPI</rdfs:comment>
	</owl:Class>
	<owl:Class rdf:about="&java-se-6;OrgOmgCORBAClassLibrary">
		<owl:equivalentClass rdf:resource="&j2se-5_0;OrgOmgCORBAClassLibrary"/>
		<rdfs:subClassOf rdf:resource="&java;JavaClassLibrary"/>
		<rdfs:comment xml:lang="en">JavaLibrary implementing the org.omg.CORBA package for Java SE 6</rdfs:comment>
		<rdfs:comment xml:lang="OWLManchester">platform:implementsInterface some OrgOmgCORBAAPI</rdfs:comment>
	</owl:Class>
	<owl:Class rdf:about="&java-se-6;OrgOmgCORBAPortableClassLibrary">
		<owl:equivalentClass rdf:resource="&j2se-5_0;OrgOmgCORBAPortableClassLibrary"/>
		<rdfs:subClassOf rdf:resource="&java;JavaClassLibrary"/>
		<rdfs:comment xml:lang="en">JavaLibrary implementing the org.omg.CORBA.portable package for Java SE 6</rdfs:comment>
		<rdfs:comment xml:lang="OWLManchester">platform:implementsInterface some OrgOmgCORBAPortableAPI</rdfs:comment>
	</owl:Class>
	<owl:Class rdf:about="&java-se-6;OrgOmgCORBADynAnyPackageClassLibrary">
		<owl:equivalentClass rdf:resource="&j2se-5_0;OrgOmgCORBADynAnyPackageClassLibrary"/>
		<rdfs:subClassOf rdf:resource="&java;JavaClassLibrary"/>
		<rdfs:comment xml:lang="en">JavaLibrary implementing the org.omg.CORBA.DynAnyPackage package for Java SE 6</rdfs:comment>
		<rdfs:comment xml:lang="OWLManchester">platform:implementsInterface some OrgOmgCORBADynAnyPackageAPI</rdfs:comment>
	</owl:Class>
	<owl:Class rdf:about="&java-se-6;OrgOmgCORBAORBPackageClassLibrary">
		<owl:equivalentClass rdf:resource="&j2se-5_0;OrgOmgCORBAORBPackageClassLibrary"/>
		<rdfs:subClassOf rdf:resource="&java;JavaClassLibrary"/>
		<rdfs:comment xml:lang="en">JavaLibrary implementing the org.omg.CORBA.ORBPackage package for Java SE 6</rdfs:comment>
		<rdfs:comment xml:lang="OWLManchester">platform:implementsInterface some OrgOmgCORBAORBPackageAPI</rdfs:comment>
	</owl:Class>
	<owl:Class rdf:about="&java-se-6;OrgOmgCORBATypeCodePackageClassLibrary">
		<owl:equivalentClass rdf:resource="&j2se-5_0;OrgOmgCORBATypeCodePackageClassLibrary"/>
		<rdfs:subClassOf rdf:resource="&java;JavaClassLibrary"/>
		<rdfs:comment xml:lang="en">JavaLibrary implementing the org.omg.CORBA.TypeCodePackage package for Java SE 6</rdfs:comment>
		<rdfs:comment xml:lang="OWLManchester">platform:implementsInterface some OrgOmgCORBATypeCodePackageAPI</rdfs:comment>
	</owl:Class>
	<owl:Class rdf:about="&java-se-6;OrgOmgSendingContextClassLibrary">
		<owl:equivalentClass rdf:resource="&j2se-5_0;OrgOmgSendingContextClassLibrary"/>
		<rdfs:subClassOf rdf:resource="&java;JavaClassLibrary"/>
		<rdfs:comment xml:lang="en">JavaLibrary implementing the org.omg.SendingContext package for Java SE 6</rdfs:comment>
		<rdfs:comment xml:lang="OWLManchester">platform:implementsInterface some OrgOmgSendingContextAPI</rdfs:comment>
	</owl:Class>
	<owl:Class rdf:about="&java-se-6;OrgOmgCosNamingClassLibrary">
		<owl:equivalentClass rdf:resource="&j2se-5_0;OrgOmgCosNamingClassLibrary"/>
		<rdfs:subClassOf rdf:resource="&java;JavaClassLibrary"/>
		<rdfs:comment xml:lang="en">JavaLibrary implementing the org.omg.CosNaming package for Java SE 6</rdfs:comment>
		<rdfs:comment xml:lang="OWLManchester">platform:implementsInterface some OrgOmgCosNamingAPI</rdfs:comment>
	</owl:Class>
	<owl:Class rdf:about="&java-se-6;OrgOmgCosNamingNamingContextExtPackageClassLibrary">
		<owl:equivalentClass rdf:resource="&j2se-5_0;OrgOmgCosNamingNamingContextExtPackageClassLibrary"/>
		<rdfs:subClassOf rdf:resource="&java;JavaClassLibrary"/>
		<rdfs:comment xml:lang="en">JavaLibrary implementing the org.omg.CosNaming.NamingContextExtPackage package for Java SE 6</rdfs:comment>
		<rdfs:comment xml:lang="OWLManchester">platform:implementsInterface some OrgOmgCosNamingNamingContextExtPackageAPI</rdfs:comment>
	</owl:Class>
	<owl:Class rdf:about="&java-se-6;OrgOmgCosNamingNamingContextPackageClassLibrary">
		<owl:equivalentClass rdf:resource="&j2se-5_0;OrgOmgCosNamingNamingContextPackageClassLibrary"/>
		<rdfs:subClassOf rdf:resource="&java;JavaClassLibrary"/>
		<rdfs:comment xml:lang="en">JavaLibrary implementing the org.omg.CosNaming.NamingContextPackage package for Java SE 6</rdfs:comment>
		<rdfs:comment xml:lang="OWLManchester">platform:implementsInterface some OrgOmgCosNamingNamingContextPackageAPI</rdfs:comment>
	</owl:Class>
	<owl:Class rdf:about="&java-se-6;OrgOmgPortableServerClassLibrary">
		<owl:equivalentClass rdf:resource="&j2se-5_0;OrgOmgPortableServerClassLibrary"/>
		<rdfs:subClassOf rdf:resource="&java;JavaClassLibrary"/>
		<rdfs:comment xml:lang="en">JavaLibrary implementing the org.omg.PortableServer package for Java SE 6</rdfs:comment>
		<rdfs:comment xml:lang="OWLManchester">platform:implementsInterface some OrgOmgPortableServerAPI</rdfs:comment>
	</owl:Class>
	<owl:Class rdf:about="&java-se-6;OrgOmgPortableServerCurrentPackageClassLibrary">
		<owl:equivalentClass rdf:resource="&j2se-5_0;OrgOmgPortableServerCurrentPackageClassLibrary"/>
		<rdfs:subClassOf rdf:resource="&java;JavaClassLibrary"/>
		<rdfs:comment xml:lang="en">JavaLibrary implementing the org.omg.PortableServer.CurrentPackage package for Java SE 6</rdfs:comment>
		<rdfs:comment xml:lang="OWLManchester">platform:implementsInterface some OrgOmgPortableServerCurrentPackageAPI</rdfs:comment>
	</owl:Class>
	<owl:Class rdf:about="&java-se-6;OrgOmgPortableServerPOAManagerPackageClassLibrary">
		<owl:equivalentClass rdf:resource="&j2se-5_0;OrgOmgPortableServerPOAManagerPackageClassLibrary"/>
		<rdfs:subClassOf rdf:resource="&java;JavaClassLibrary"/>
		<rdfs:comment xml:lang="en">JavaLibrary implementing the org.omg.PortableServer.POAManagerPackage package for Java SE 6</rdfs:comment>
		<rdfs:comment xml:lang="OWLManchester">platform:implementsInterface some OrgOmgPortableServerPOAManagerPackageAPI</rdfs:comment>
	</owl:Class>
	<owl:Class rdf:about="&java-se-6;OrgOmgPortableServerPOAPackageClassLibrary">
		<owl:equivalentClass rdf:resource="&j2se-5_0;OrgOmgPortableServerPOAPackageClassLibrary"/>
		<rdfs:subClassOf rdf:resource="&java;JavaClassLibrary"/>
		<rdfs:comment xml:lang="en">JavaLibrary implementing the org.omg.PortableServer.POAPackage package for Java SE 6</rdfs:comment>
		<rdfs:comment xml:lang="OWLManchester">platform:implementsInterface some OrgOmgPortableServerPOAPackageAPI</rdfs:comment>
	</owl:Class>
	<owl:Class rdf:about="&java-se-6;OrgOmgPortableServerPortableClassLibrary">
		<owl:equivalentClass rdf:resource="&j2se-5_0;OrgOmgPortableServerPortableClassLibrary"/>
		<rdfs:subClassOf rdf:resource="&java;JavaClassLibrary"/>
		<rdfs:comment xml:lang="en">JavaLibrary implementing the org.omg.PortableServer.portable package for Java SE 6</rdfs:comment>
		<rdfs:comment xml:lang="OWLManchester">platform:implementsInterface some OrgOmgPortableServerPortableAPI</rdfs:comment>
	</owl:Class>
	<owl:Class rdf:about="&java-se-6;OrgOmgPortableServerServantLocatorPackageClassLibrary">
		<owl:equivalentClass rdf:resource="&j2se-5_0;OrgOmgPortableServerServantLocatorPackageClassLibrary"/>
		<rdfs:subClassOf rdf:resource="&java;JavaClassLibrary"/>
		<rdfs:comment xml:lang="en">JavaLibrary implementing the org.omg.PortableServer.ServantLocatorPackage package for Java SE 6</rdfs:comment>
		<rdfs:comment xml:lang="OWLManchester">platform:implementsInterface some OrgOmgPortableServerServantLocatorPackageAPI</rdfs:comment>
	</owl:Class>
	<owl:Class rdf:about="&java-se-6;OrgOmgDynamicClassLibrary">
		<owl:equivalentClass rdf:resource="&j2se-5_0;OrgOmgDynamicClassLibrary"/>
		<rdfs:subClassOf rdf:resource="&java;JavaClassLibrary"/>
		<rdfs:comment xml:lang="en">JavaLibrary implementing the org.omg.Dynamic package for Java SE 6</rdfs:comment>
		<rdfs:comment xml:lang="OWLManchester">platform:implementsInterface some OrgOmgDynamicAPI</rdfs:comment>
	</owl:Class>
	<owl:Class rdf:about="&java-se-6;OrgOmgDynamicAnyClassLibrary">
		<owl:equivalentClass rdf:resource="&j2se-5_0;OrgOmgDynamicAnyClassLibrary"/>
		<rdfs:subClassOf rdf:resource="&java;JavaClassLibrary"/>
		<rdfs:comment xml:lang="en">JavaLibrary implementing the org.omg.DynamicAny package for Java SE 6</rdfs:comment>
		<rdfs:comment xml:lang="OWLManchester">platform:implementsInterface some OrgOmgDynamicAnyAPI</rdfs:comment>
	</owl:Class>
	<owl:Class rdf:about="&java-se-6;OrgOmgDynamicAnyDynAnyFactoryPackageClassLibrary">
		<owl:equivalentClass rdf:resource="&j2se-5_0;OrgOmgDynamicAnyDynAnyFactoryPackageClassLibrary"/>
		<rdfs:subClassOf rdf:resource="&java;JavaClassLibrary"/>
		<rdfs:comment xml:lang="en">JavaLibrary implementing the org.omg.DynamicAny.DynAnyFactoryPackage package for Java SE 6</rdfs:comment>
		<rdfs:comment xml:lang="OWLManchester">platform:implementsInterface some OrgOmgDynamicAnyDynAnyFactoryPackageAPI</rdfs:comment>
	</owl:Class>
	<owl:Class rdf:about="&java-se-6;OrgOmgDynamicAnyDynAnyPackageClassLibrary">
		<owl:equivalentClass rdf:resource="&j2se-5_0;OrgOmgDynamicAnyDynAnyPackageClassLibrary"/>
		<rdfs:subClassOf rdf:resource="&java;JavaClassLibrary"/>
		<rdfs:comment xml:lang="en">JavaLibrary implementing the org.omg.DynamicAny.DynAnyPackage package for Java SE 6</rdfs:comment>
		<rdfs:comment xml:lang="OWLManchester">platform:implementsInterface some OrgOmgDynamicAnyDynAnyPackageAPI</rdfs:comment>
	</owl:Class>
	<owl:Class rdf:about="&java-se-6;OrgOmgIOPClassLibrary">
		<owl:equivalentClass rdf:resource="&j2se-5_0;OrgOmgIOPClassLibrary"/>
		<rdfs:subClassOf rdf:resource="&java;JavaClassLibrary"/>
		<rdfs:comment xml:lang="en">JavaLibrary implementing the org.omg.IOP package for Java SE 6</rdfs:comment>
		<rdfs:comment xml:lang="OWLManchester">platform:implementsInterface some OrgOmgIOPAPI</rdfs:comment>
	</owl:Class>
	<owl:Class rdf:about="&java-se-6;OrgOmgIOPCodecFactoryPackageClassLibrary">
		<owl:equivalentClass rdf:resource="&j2se-5_0;OrgOmgIOPCodecFactoryPackageClassLibrary"/>
		<rdfs:subClassOf rdf:resource="&java;JavaClassLibrary"/>
		<rdfs:comment xml:lang="en">JavaLibrary implementing the org.omg.IOP.CodecFactoryPackage package for Java SE 6</rdfs:comment>
		<rdfs:comment xml:lang="OWLManchester">platform:implementsInterface some OrgOmgIOPCodecFactoryPackageAPI</rdfs:comment>
	</owl:Class>
	<owl:Class rdf:about="&java-se-6;OrgOmgIOPCodecPackageClassLibrary">
		<owl:equivalentClass rdf:resource="&j2se-5_0;OrgOmgIOPCodecPackageClassLibrary"/>
		<rdfs:subClassOf rdf:resource="&java;JavaClassLibrary"/>
		<rdfs:comment xml:lang="en">JavaLibrary implementing the org.omg.IOP.CodecPackage package for Java SE 6</rdfs:comment>
		<rdfs:comment xml:lang="OWLManchester">platform:implementsInterface some OrgOmgIOPCodecPackageAPI</rdfs:comment>
	</owl:Class>
	<owl:Class rdf:about="&java-se-6;OrgOmgMessagingClassLibrary">
		<owl:equivalentClass rdf:resource="&j2se-5_0;OrgOmgMessagingClassLibrary"/>
		<rdfs:subClassOf rdf:resource="&java;JavaClassLibrary"/>
		<rdfs:comment xml:lang="en">JavaLibrary implementing the org.omg.Messaging package for Java SE 6</rdfs:comment>
		<rdfs:comment xml:lang="OWLManchester">platform:implementsInterface some OrgOmgMessagingAPI</rdfs:comment>
	</owl:Class>
	<owl:Class rdf:about="&java-se-6;OrgOmgPortableInterceptorClassLibrary">
		<owl:equivalentClass rdf:resource="&j2se-5_0;OrgOmgPortableInterceptorClassLibrary"/>
		<rdfs:subClassOf rdf:resource="&java;JavaClassLibrary"/>
		<rdfs:comment xml:lang="en">JavaLibrary implementing the org.omg.PortableInterceptor package for Java SE 6</rdfs:comment>
		<rdfs:comment xml:lang="OWLManchester">platform:implementsInterface some OrgOmgPortableInterceptorAPI</rdfs:comment>
	</owl:Class>
	<owl:Class rdf:about="&java-se-6;OrgOmgPortableInterceptorORBInitInfoPackageClassLibrary">
		<owl:equivalentClass rdf:resource="&j2se-5_0;OrgOmgPortableInterceptorORBInitInfoPackageClassLibrary"/>
		<rdfs:subClassOf rdf:resource="&java;JavaClassLibrary"/>
		<rdfs:comment xml:lang="en">JavaLibrary implementing the org.omg.PortableInterceptor.ORBInitInfoPackage package for Java SE 6</rdfs:comment>
		<rdfs:comment xml:lang="OWLManchester">platform:implementsInterface some OrgOmgPortableInterceptorORBInitInfoPackageAPI</rdfs:comment>
	</owl:Class>
	<owl:Class rdf:about="&java-se-6;OrgOmgStubJavaRmiClassLibrary">
		<owl:equivalentClass rdf:resource="&j2se-5_0;OrgOmgStubJavaRmiClassLibrary"/>
		<rdfs:subClassOf rdf:resource="&java;JavaClassLibrary"/>
		<rdfs:comment xml:lang="en">JavaLibrary implementing the org.omg.stub.java.rmi package for Java SE 6</rdfs:comment>
		<rdfs:comment xml:lang="OWLManchester">platform:implementsInterface some OrgOmgStubJavaRmiAPI</rdfs:comment>
	</owl:Class>
	<owl:Class rdf:about="&java-se-6;OrgOmgStubJavaxManagementRemoteRmiClassLibrary">
		<owl:equivalentClass rdf:resource="&j2se-5_0;OrgOmgStubJavaxManagementRemoteRmiClassLibrary"/>
		<rdfs:subClassOf rdf:resource="&java;JavaClassLibrary"/>
		<rdfs:comment xml:lang="en">JavaLibrary implementing the org.omg.stub.javax.management.remote.rmi package for Java SE 6</rdfs:comment>
		<rdfs:comment xml:lang="OWLManchester">platform:implementsInterface some OrgOmgStubJavaxManagementRemoteRmiAPI</rdfs:comment>
	</owl:Class>
	<owl:Class rdf:about="&java-se-6;OrgXmlSaxClassLibrary">
		<owl:equivalentClass rdf:resource="&j2se-5_0;OrgXmlSaxClassLibrary"/>
		<rdfs:subClassOf rdf:resource="&java;JavaClassLibrary"/>
		<rdfs:comment xml:lang="en">JavaLibrary implementing the org.xml.sax package for Java SE 6</rdfs:comment>
		<rdfs:comment xml:lang="OWLManchester">platform:implementsInterface some OrgXmlSaxAPI</rdfs:comment>
	</owl:Class>
	<owl:Class rdf:about="&java-se-6;OrgXmlSaxHelpersClassLibrary">
		<owl:equivalentClass rdf:resource="&j2se-5_0;OrgXmlSaxHelpersClassLibrary"/>
		<rdfs:subClassOf rdf:resource="&java;JavaClassLibrary"/>
		<rdfs:comment xml:lang="en">JavaLibrary implementing the org.xml.sax.helpers package for Java SE 6</rdfs:comment>
		<rdfs:comment xml:lang="OWLManchester">platform:implementsInterface some OrgXmlSaxHelpersAPI</rdfs:comment>
	</owl:Class>
	<owl:Class rdf:about="&java-se-6;OrgXmlSaxExtClassLibrary">
		<owl:equivalentClass rdf:resource="&j2se-5_0;OrgXmlSaxExtClassLibrary"/>
		<rdfs:subClassOf rdf:resource="&java;JavaClassLibrary"/>
		<rdfs:comment xml:lang="en">JavaLibrary implementing the org.xml.sax.ext package for Java SE 6</rdfs:comment>
		<rdfs:comment xml:lang="OWLManchester">platform:implementsInterface some OrgXmlSaxExtAPI</rdfs:comment>
	</owl:Class>
	<owl:Class rdf:about="&java-se-6;OrgIetfJgssClassLibrary">
		<owl:equivalentClass rdf:resource="&j2se-5_0;OrgIetfJgssClassLibrary"/>
		<rdfs:subClassOf rdf:resource="&java;JavaClassLibrary"/>
		<rdfs:comment xml:lang="en">JavaLibrary implementing the org.ietf.jgss package for Java SE 6</rdfs:comment>
		<rdfs:comment xml:lang="OWLManchester">platform:implementsInterface some OrgIetfJgssAPI</rdfs:comment>
	</owl:Class>
</rdf:RDF>
