<?xml version="1.0" encoding="ISO-8859-1"?>
<!DOCTYPE rdf:RDF [
	<!ENTITY isa "http://localhost/~dennis/platformkit/2010_1/isa.owl#">
	<!ENTITY jdk-1_1 "http://soft.vub.ac.be/platformkit/2010/1/jdk-1_1.owl#">
	<!ENTITY platform "http://localhost/~dennis/platformkit/2010_1/platform.owl#">
	<!ENTITY ns_19 "http://localhost/~dennis/platformkit/2010_1/">
	<!ENTITY personaljava-1_1 "http://soft.vub.ac.be/platformkit/2010/1/personaljava-1_1.owl#">
	<!ENTITY java "http://localhost/~dennis/platformkit/2010_1/java.owl#">
	<!ENTITY xsd "http://www.w3.org/2001/XMLSchema#">
	<!ENTITY owl "http://www.w3.org/2002/07/owl#">
	<!ENTITY rdf "http://www.w3.org/1999/02/22-rdf-syntax-ns#">
	<!ENTITY rdfs "http://www.w3.org/2000/01/rdf-schema#">
]>
<rdf:RDF
	 xmlns:isa="&isa;"
	 xmlns:jdk-1_1="&jdk-1_1;"
	 xmlns:platform="&platform;"
	 xmlns:ns_19="&ns_19;"
	 xmlns:personaljava-1_1="&personaljava-1_1;"
	 xmlns:java="&java;"
	 xmlns:xsd="&xsd;"
	 xmlns:owl="&owl;"
	 xmlns:rdf="&rdf;"
	 xmlns:rdfs="&rdfs;"
>

	<owl:Ontology rdf:about="http://soft.vub.ac.be/platformkit/2010/1/jdk-1_1.owl#">
		<owl:versionInfo>$Id: UML2ToPackageAPIOntology.atl 8082 2010-03-18 21:11:00Z dwagelaa $</owl:versionInfo>
		<owl:imports rdf:resource="http://localhost/~dennis/platformkit/2010_1/platform.owl"/>
		<owl:imports rdf:resource="http://localhost/~dennis/platformkit/2010_1/java.owl"/>
		<owl:imports rdf:resource="http://soft.vub.ac.be/platformkit/2010/1/personaljava-1_1.owl#"/>
		<owl:imports rdf:resource="http://localhost/~dennis/platformkit/2010_1/isa.owl"/>
		<rdfs:comment xml:lang="en">Generated by [UML2ToSimplifiedPackageAPIOntology.atl 8080 2010-03-18 10:46:40Z dwagelaa], [UML2ToPackageAPIOntology.atl 8082 2010-03-18 21:11:00Z dwagelaa], [UML2ToAPIOntology.atl 8082 2010-03-18 21:11:00Z dwagelaa], and [UML2Comparison.atl 8082 2010-03-18 21:11:00Z dwagelaa]</rdfs:comment>
		<rdfs:comment>Dennis Wagelaar &lt;dennis.wagelaar@vub.ac.be&gt;</rdfs:comment>
		<rdfs:comment xml:lang="en">&#169; 2010, Vrije Universiteit Brussel. All rights reserved.</rdfs:comment>
		<rdfs:label xml:lang="en">JDK 1.1</rdfs:label>
	</owl:Ontology>
	<owl:Class rdf:about="&jdk-1_1;JDK1_1API">
		<rdfs:subClassOf rdf:resource="&jdk-1_1;JavaLangAPI"/>
		<rdfs:subClassOf rdf:resource="&jdk-1_1;JavaLangReflectAPI"/>
		<rdfs:subClassOf rdf:resource="&jdk-1_1;JavaIoAPI"/>
		<rdfs:subClassOf rdf:resource="&jdk-1_1;JavaNetAPI"/>
		<rdfs:subClassOf rdf:resource="&jdk-1_1;JavaUtilAPI"/>
		<rdfs:subClassOf rdf:resource="&jdk-1_1;JavaUtilZipAPI"/>
		<rdfs:subClassOf rdf:resource="&jdk-1_1;JavaTextAPI"/>
		<rdfs:subClassOf rdf:resource="&jdk-1_1;JavaTextResourcesAPI"/>
		<rdfs:subClassOf rdf:resource="&jdk-1_1;JavaMathAPI"/>
		<rdfs:subClassOf rdf:resource="&jdk-1_1;JavaSecurityAPI"/>
		<rdfs:subClassOf rdf:resource="&jdk-1_1;JavaSecurityAclAPI"/>
		<rdfs:subClassOf rdf:resource="&jdk-1_1;JavaSecurityInterfacesAPI"/>
		<rdfs:subClassOf rdf:resource="&jdk-1_1;JavaAwtAPI"/>
		<rdfs:subClassOf rdf:resource="&jdk-1_1;JavaAwtImageAPI"/>
		<rdfs:subClassOf rdf:resource="&jdk-1_1;JavaAwtDatatransferAPI"/>
		<rdfs:subClassOf rdf:resource="&jdk-1_1;JavaAwtEventAPI"/>
		<rdfs:subClassOf rdf:resource="&jdk-1_1;JavaAppletAPI"/>
		<rdfs:subClassOf rdf:resource="&jdk-1_1;JavaSqlAPI"/>
		<rdfs:subClassOf rdf:resource="&jdk-1_1;JavaRmiAPI"/>
		<rdfs:subClassOf rdf:resource="&jdk-1_1;JavaRmiRegistryAPI"/>
		<rdfs:subClassOf rdf:resource="&jdk-1_1;JavaRmiDgcAPI"/>
		<rdfs:subClassOf rdf:resource="&jdk-1_1;JavaRmiServerAPI"/>
		<rdfs:subClassOf rdf:resource="&jdk-1_1;JavaBeansAPI"/>
		<rdfs:subClassOf rdf:resource="&personaljava-1_1;PersonalJava1_1API"/>
		<rdfs:comment xml:lang="en">JDK 1.1 API</rdfs:comment>
		<rdfs:comment xml:lang="OWLManchester">platform:comprisesInterfacePart some JavaLang and platform:comprisesInterfacePart some JavaLangReflect and platform:comprisesInterfacePart some JavaIo and platform:comprisesInterfacePart some JavaNet and platform:comprisesInterfacePart some JavaUtil and platform:comprisesInterfacePart some JavaUtilZip and platform:comprisesInterfacePart some JavaText and platform:comprisesInterfacePart some JavaTextResources and platform:comprisesInterfacePart some JavaMath and platform:comprisesInterfacePart some JavaSecurity and platform:comprisesInterfacePart some JavaSecurityAcl and platform:comprisesInterfacePart some JavaSecurityInterfaces and platform:comprisesInterfacePart some JavaAwt and platform:comprisesInterfacePart some JavaAwtImage and platform:comprisesInterfacePart some JavaAwtDatatransfer and platform:comprisesInterfacePart some JavaAwtEvent and platform:comprisesInterfacePart some JavaApplet and platform:comprisesInterfacePart some JavaSql and platform:comprisesInterfacePart some JavaRmi and platform:comprisesInterfacePart some JavaRmiRegistry and platform:comprisesInterfacePart some JavaRmiDgc and platform:comprisesInterfacePart some JavaRmiServer and platform:comprisesInterfacePart some JavaBeans</rdfs:comment>
	</owl:Class>
	<owl:Class rdf:about="&jdk-1_1;JDK1_1ClassLibrary">
		<rdfs:subClassOf rdf:resource="&jdk-1_1;JavaLangClassLibrary"/>
		<rdfs:subClassOf rdf:resource="&jdk-1_1;JavaLangReflectClassLibrary"/>
		<rdfs:subClassOf rdf:resource="&jdk-1_1;JavaIoClassLibrary"/>
		<rdfs:subClassOf rdf:resource="&jdk-1_1;JavaNetClassLibrary"/>
		<rdfs:subClassOf rdf:resource="&jdk-1_1;JavaUtilClassLibrary"/>
		<rdfs:subClassOf rdf:resource="&jdk-1_1;JavaUtilZipClassLibrary"/>
		<rdfs:subClassOf rdf:resource="&jdk-1_1;JavaTextClassLibrary"/>
		<rdfs:subClassOf rdf:resource="&jdk-1_1;JavaTextResourcesClassLibrary"/>
		<rdfs:subClassOf rdf:resource="&jdk-1_1;JavaMathClassLibrary"/>
		<rdfs:subClassOf rdf:resource="&jdk-1_1;JavaSecurityClassLibrary"/>
		<rdfs:subClassOf rdf:resource="&jdk-1_1;JavaSecurityAclClassLibrary"/>
		<rdfs:subClassOf rdf:resource="&jdk-1_1;JavaSecurityInterfacesClassLibrary"/>
		<rdfs:subClassOf rdf:resource="&jdk-1_1;JavaAwtClassLibrary"/>
		<rdfs:subClassOf rdf:resource="&jdk-1_1;JavaAwtImageClassLibrary"/>
		<rdfs:subClassOf rdf:resource="&jdk-1_1;JavaAwtDatatransferClassLibrary"/>
		<rdfs:subClassOf rdf:resource="&jdk-1_1;JavaAwtEventClassLibrary"/>
		<rdfs:subClassOf rdf:resource="&jdk-1_1;JavaAppletClassLibrary"/>
		<rdfs:subClassOf rdf:resource="&jdk-1_1;JavaSqlClassLibrary"/>
		<rdfs:subClassOf rdf:resource="&jdk-1_1;JavaRmiClassLibrary"/>
		<rdfs:subClassOf rdf:resource="&jdk-1_1;JavaRmiRegistryClassLibrary"/>
		<rdfs:subClassOf rdf:resource="&jdk-1_1;JavaRmiDgcClassLibrary"/>
		<rdfs:subClassOf rdf:resource="&jdk-1_1;JavaRmiServerClassLibrary"/>
		<rdfs:subClassOf rdf:resource="&jdk-1_1;JavaBeansClassLibrary"/>
		<rdfs:subClassOf rdf:resource="&personaljava-1_1;PersonalJava1_1ClassLibrary"/>
		<rdfs:comment xml:lang="en">Java class library implementing the JDK 1.1 API</rdfs:comment>
		<rdfs:comment xml:lang="OWLManchester">platform:implementsInterface some JDK1_1API</rdfs:comment>
	</owl:Class>
	<owl:Class rdf:about="&jdk-1_1;JDK1_1BytecodeFormat">
		<owl:equivalentClass rdf:resource="&personaljava-1_1;PersonalJava1_1BytecodeFormat"/>
		<rdfs:subClassOf rdf:resource="&isa;JavaBytecode"/>
		<rdfs:comment xml:lang="en">JDK 1.1 bytecode format</rdfs:comment>
		<rdfs:comment xml:lang="OWLManchester">java:majorVersionNumber some xsd:integer[>="45"^^xsd:integer] and java:preverified value false</rdfs:comment>
	</owl:Class>
	<jdk-1_1:JDK1_1BytecodeFormat rdf:about="&jdk-1_1;theJDK1_1BytecodeFormat">
		<java:preverified rdf:datatype="http://www.w3.org/2001/XMLSchema#boolean">false</java:preverified>
		<java:minorVersionNumber rdf:datatype="http://www.w3.org/2001/XMLSchema#integer">3</java:minorVersionNumber>
		<java:majorVersionNumber rdf:datatype="http://www.w3.org/2001/XMLSchema#integer">45</java:majorVersionNumber>
	</jdk-1_1:JDK1_1BytecodeFormat>
	<jdk-1_1:JDK1_1API rdf:about="&jdk-1_1;theJDK1_1API">
		<platform:comprisesInterfacePart rdf:resource="&jdk-1_1;theJavaBeansPart"/>
		<platform:comprisesInterfacePart rdf:resource="&jdk-1_1;theJavaRmiServerPart"/>
		<platform:comprisesInterfacePart rdf:resource="&jdk-1_1;theJavaRmiDgcPart"/>
		<platform:comprisesInterfacePart rdf:resource="&jdk-1_1;theJavaRmiRegistryPart"/>
		<platform:comprisesInterfacePart rdf:resource="&jdk-1_1;theJavaRmiPart"/>
		<platform:comprisesInterfacePart rdf:resource="&jdk-1_1;theJavaSqlPart"/>
		<platform:comprisesInterfacePart rdf:resource="&jdk-1_1;theJavaAppletPart"/>
		<platform:comprisesInterfacePart rdf:resource="&jdk-1_1;theJavaAwtEventPart"/>
		<platform:comprisesInterfacePart rdf:resource="&jdk-1_1;theJavaAwtDatatransferPart"/>
		<platform:comprisesInterfacePart rdf:resource="&jdk-1_1;theJavaAwtImagePart"/>
		<platform:comprisesInterfacePart rdf:resource="&jdk-1_1;theJavaAwtPart"/>
		<platform:comprisesInterfacePart rdf:resource="&jdk-1_1;theJavaSecurityInterfacesPart"/>
		<platform:comprisesInterfacePart rdf:resource="&jdk-1_1;theJavaSecurityAclPart"/>
		<platform:comprisesInterfacePart rdf:resource="&jdk-1_1;theJavaSecurityPart"/>
		<platform:comprisesInterfacePart rdf:resource="&jdk-1_1;theJavaMathPart"/>
		<platform:comprisesInterfacePart rdf:resource="&jdk-1_1;theJavaTextResourcesPart"/>
		<platform:comprisesInterfacePart rdf:resource="&jdk-1_1;theJavaTextPart"/>
		<platform:comprisesInterfacePart rdf:resource="&jdk-1_1;theJavaUtilZipPart"/>
		<platform:comprisesInterfacePart rdf:resource="&jdk-1_1;theJavaUtilPart"/>
		<platform:comprisesInterfacePart rdf:resource="&jdk-1_1;theJavaNetPart"/>
		<platform:comprisesInterfacePart rdf:resource="&jdk-1_1;theJavaIoPart"/>
		<platform:comprisesInterfacePart rdf:resource="&jdk-1_1;theJavaLangReflectPart"/>
		<platform:comprisesInterfacePart rdf:resource="&jdk-1_1;theJavaLangPart"/>
	</jdk-1_1:JDK1_1API>
	<owl:Class rdf:about="&jdk-1_1;JDK1_1VM">
		<owl:equivalentClass>
			<owl:Restriction>
				<owl:onProperty rdf:resource="&platform;implementsInterface"/>
				<owl:someValuesFrom rdf:resource="&jdk-1_1;JDK1_1BytecodeFormat"/>
			</owl:Restriction>
		</owl:equivalentClass>
		<rdfs:subClassOf rdf:resource="&java;JavaVM"/>
		<rdfs:comment xml:lang="en">JDK 1.1 virtual machine</rdfs:comment>
	</owl:Class>
	<owl:Class rdf:about="&jdk-1_1;JDK1_1JRE">
		<owl:equivalentClass>
			<owl:Class >
				<owl:intersectionOf rdf:parseType="Collection">
					<owl:Restriction>
						<owl:onProperty rdf:resource="&platform;providesFeature"/>
						<owl:someValuesFrom rdf:resource="&jdk-1_1;JDK1_1ClassLibrary"/>
					</owl:Restriction>
					<owl:Restriction>
						<owl:onProperty rdf:resource="&platform;providesFeature"/>
						<owl:someValuesFrom rdf:resource="&jdk-1_1;JDK1_1VM"/>
					</owl:Restriction>
				</owl:intersectionOf>
			</owl:Class>
		</owl:equivalentClass>
		<rdfs:subClassOf rdf:resource="&java;JRE"/>
		<rdfs:comment xml:lang="en">JDK 1.1 Java Runtime Environment</rdfs:comment>
	</owl:Class>
	<owl:Class rdf:about="&jdk-1_1;JavaLang">
		<owl:equivalentClass rdf:resource="&personaljava-1_1;JavaLang"/>
		<rdfs:subClassOf rdf:resource="&java;JavaAPIPart"/>
		<rdfs:seeAlso rdf:resource="&jdk-1_1;JavaUtil"/>
		<rdfs:seeAlso rdf:resource="&jdk-1_1;JavaLangReflect"/>
		<rdfs:seeAlso rdf:resource="&jdk-1_1;JavaNet"/>
		<rdfs:seeAlso rdf:resource="&jdk-1_1;JavaIo"/>
		<rdfs:comment xml:lang="en">Java API part implementing the java.lang package for JDK 1.1</rdfs:comment>
	</owl:Class>
	<owl:Class rdf:about="&jdk-1_1;JavaLangReflect">
		<owl:equivalentClass rdf:resource="&personaljava-1_1;JavaLangReflect"/>
		<rdfs:subClassOf rdf:resource="&java;JavaAPIPart"/>
		<rdfs:seeAlso rdf:resource="&jdk-1_1;JavaLang"/>
		<rdfs:comment xml:lang="en">Java API part implementing the java.lang.reflect package for JDK 1.1</rdfs:comment>
	</owl:Class>
	<owl:Class rdf:about="&jdk-1_1;JavaIo">
		<rdfs:subClassOf rdf:resource="&personaljava-1_1;JavaIo"/>
		<rdfs:seeAlso rdf:resource="&jdk-1_1;JavaLang"/>
		<rdfs:seeAlso rdf:resource="&jdk-1_1;JavaUtil"/>
		<rdfs:comment xml:lang="en">Java API part implementing the java.io package for JDK 1.1</rdfs:comment>
	</owl:Class>
	<owl:Class rdf:about="&jdk-1_1;JavaNet">
		<owl:equivalentClass rdf:resource="&personaljava-1_1;JavaNet"/>
		<rdfs:subClassOf rdf:resource="&java;JavaAPIPart"/>
		<rdfs:seeAlso rdf:resource="&jdk-1_1;JavaLang"/>
		<rdfs:seeAlso rdf:resource="&jdk-1_1;JavaIo"/>
		<rdfs:comment xml:lang="en">Java API part implementing the java.net package for JDK 1.1</rdfs:comment>
	</owl:Class>
	<owl:Class rdf:about="&jdk-1_1;JavaUtil">
		<owl:equivalentClass rdf:resource="&personaljava-1_1;JavaUtil"/>
		<rdfs:subClassOf rdf:resource="&java;JavaAPIPart"/>
		<rdfs:seeAlso rdf:resource="&jdk-1_1;JavaLang"/>
		<rdfs:seeAlso rdf:resource="&jdk-1_1;JavaIo"/>
		<rdfs:comment xml:lang="en">Java API part implementing the java.util package for JDK 1.1</rdfs:comment>
	</owl:Class>
	<owl:Class rdf:about="&jdk-1_1;JavaUtilZip">
		<rdfs:subClassOf rdf:resource="&personaljava-1_1;JavaUtilZip"/>
		<rdfs:seeAlso rdf:resource="&jdk-1_1;JavaLang"/>
		<rdfs:seeAlso rdf:resource="&jdk-1_1;JavaUtil"/>
		<rdfs:seeAlso rdf:resource="&jdk-1_1;JavaIo"/>
		<rdfs:comment xml:lang="en">Java API part implementing the java.util.zip package for JDK 1.1</rdfs:comment>
	</owl:Class>
	<owl:Class rdf:about="&jdk-1_1;JavaText">
		<owl:equivalentClass rdf:resource="&personaljava-1_1;JavaText"/>
		<rdfs:subClassOf rdf:resource="&java;JavaAPIPart"/>
		<rdfs:seeAlso rdf:resource="&jdk-1_1;JavaLang"/>
		<rdfs:seeAlso rdf:resource="&jdk-1_1;JavaUtil"/>
		<rdfs:seeAlso rdf:resource="&jdk-1_1;JavaIo"/>
		<rdfs:comment xml:lang="en">Java API part implementing the java.text package for JDK 1.1</rdfs:comment>
	</owl:Class>
	<owl:Class rdf:about="&jdk-1_1;JavaTextResources">
		<rdfs:subClassOf rdf:resource="&personaljava-1_1;JavaTextResources"/>
		<rdfs:seeAlso rdf:resource="&jdk-1_1;JavaLang"/>
		<rdfs:seeAlso rdf:resource="&jdk-1_1;JavaUtil"/>
		<rdfs:comment xml:lang="en">Java API part implementing the java.text.resources package for JDK 1.1</rdfs:comment>
	</owl:Class>
	<owl:Class rdf:about="&jdk-1_1;JavaMath">
		<rdfs:subClassOf rdf:resource="&java;JavaAPIPart"/>
		<rdfs:seeAlso rdf:resource="&jdk-1_1;JavaLang"/>
		<rdfs:seeAlso rdf:resource="&jdk-1_1;JavaUtil"/>
		<rdfs:comment xml:lang="en">Java API part implementing the java.math package for JDK 1.1</rdfs:comment>
	</owl:Class>
	<owl:Class rdf:about="&jdk-1_1;JavaSecurity">
		<rdfs:subClassOf rdf:resource="&java;JavaAPIPart"/>
		<rdfs:seeAlso rdf:resource="&jdk-1_1;JavaUtil"/>
		<rdfs:seeAlso rdf:resource="&jdk-1_1;JavaLang"/>
		<rdfs:seeAlso rdf:resource="&jdk-1_1;JavaIo"/>
		<rdfs:comment xml:lang="en">Java API part implementing the java.security package for JDK 1.1</rdfs:comment>
	</owl:Class>
	<owl:Class rdf:about="&jdk-1_1;JavaSecurityAcl">
		<rdfs:subClassOf rdf:resource="&java;JavaAPIPart"/>
		<rdfs:seeAlso rdf:resource="&jdk-1_1;JavaLang"/>
		<rdfs:seeAlso rdf:resource="&jdk-1_1;JavaSecurity"/>
		<rdfs:seeAlso rdf:resource="&jdk-1_1;JavaUtil"/>
		<rdfs:comment xml:lang="en">Java API part implementing the java.security.acl package for JDK 1.1</rdfs:comment>
	</owl:Class>
	<owl:Class rdf:about="&jdk-1_1;JavaSecurityInterfaces">
		<rdfs:subClassOf rdf:resource="&java;JavaAPIPart"/>
		<rdfs:seeAlso rdf:resource="&jdk-1_1;JavaSecurity"/>
		<rdfs:seeAlso rdf:resource="&jdk-1_1;JavaMath"/>
		<rdfs:comment xml:lang="en">Java API part implementing the java.security.interfaces package for JDK 1.1</rdfs:comment>
	</owl:Class>
	<owl:Class rdf:about="&jdk-1_1;JavaAwt">
		<rdfs:subClassOf rdf:resource="&personaljava-1_1;JavaAwt"/>
		<rdfs:seeAlso rdf:resource="&jdk-1_1;JavaAwtEvent"/>
		<rdfs:seeAlso rdf:resource="&jdk-1_1;JavaIo"/>
		<rdfs:seeAlso rdf:resource="&jdk-1_1;JavaAwtImage"/>
		<rdfs:seeAlso rdf:resource="&jdk-1_1;JavaUtil"/>
		<rdfs:seeAlso rdf:resource="&jdk-1_1;JavaLang"/>
		<rdfs:seeAlso rdf:resource="&jdk-1_1;JavaNet"/>
		<rdfs:seeAlso rdf:resource="&jdk-1_1;JavaAwtDatatransfer"/>
		<rdfs:comment xml:lang="en">Java API part implementing the java.awt package for JDK 1.1</rdfs:comment>
	</owl:Class>
	<owl:Class rdf:about="&jdk-1_1;JavaAwtImage">
		<owl:equivalentClass rdf:resource="&personaljava-1_1;JavaAwtImage"/>
		<rdfs:subClassOf rdf:resource="&java;JavaAPIPart"/>
		<rdfs:seeAlso rdf:resource="&jdk-1_1;JavaLang"/>
		<rdfs:seeAlso rdf:resource="&jdk-1_1;JavaUtil"/>
		<rdfs:seeAlso rdf:resource="&jdk-1_1;JavaAwt"/>
		<rdfs:comment xml:lang="en">Java API part implementing the java.awt.image package for JDK 1.1</rdfs:comment>
	</owl:Class>
	<owl:Class rdf:about="&jdk-1_1;JavaAwtDatatransfer">
		<owl:equivalentClass rdf:resource="&personaljava-1_1;JavaAwtDatatransfer"/>
		<rdfs:subClassOf rdf:resource="&java;JavaAPIPart"/>
		<rdfs:seeAlso rdf:resource="&jdk-1_1;JavaLang"/>
		<rdfs:comment xml:lang="en">Java API part implementing the java.awt.datatransfer package for JDK 1.1</rdfs:comment>
	</owl:Class>
	<owl:Class rdf:about="&jdk-1_1;JavaAwtEvent">
		<owl:equivalentClass rdf:resource="&personaljava-1_1;JavaAwtEvent"/>
		<rdfs:subClassOf rdf:resource="&java;JavaAPIPart"/>
		<rdfs:seeAlso rdf:resource="&jdk-1_1;JavaLang"/>
		<rdfs:seeAlso rdf:resource="&jdk-1_1;JavaUtil"/>
		<rdfs:seeAlso rdf:resource="&jdk-1_1;JavaAwt"/>
		<rdfs:comment xml:lang="en">Java API part implementing the java.awt.event package for JDK 1.1</rdfs:comment>
	</owl:Class>
	<owl:Class rdf:about="&jdk-1_1;JavaApplet">
		<owl:equivalentClass rdf:resource="&personaljava-1_1;JavaApplet"/>
		<rdfs:subClassOf rdf:resource="&java;JavaAPIPart"/>
		<rdfs:seeAlso rdf:resource="&jdk-1_1;JavaLang"/>
		<rdfs:seeAlso rdf:resource="&jdk-1_1;JavaUtil"/>
		<rdfs:seeAlso rdf:resource="&jdk-1_1;JavaNet"/>
		<rdfs:seeAlso rdf:resource="&jdk-1_1;JavaAwt"/>
		<rdfs:comment xml:lang="en">Java API part implementing the java.applet package for JDK 1.1</rdfs:comment>
	</owl:Class>
	<owl:Class rdf:about="&jdk-1_1;JavaSql">
		<rdfs:subClassOf rdf:resource="&java;JavaAPIPart"/>
		<rdfs:seeAlso rdf:resource="&jdk-1_1;JavaLang"/>
		<rdfs:seeAlso rdf:resource="&jdk-1_1;JavaUtil"/>
		<rdfs:seeAlso rdf:resource="&jdk-1_1;JavaMath"/>
		<rdfs:seeAlso rdf:resource="&jdk-1_1;JavaIo"/>
		<rdfs:comment xml:lang="en">Java API part implementing the java.sql package for JDK 1.1</rdfs:comment>
	</owl:Class>
	<owl:Class rdf:about="&jdk-1_1;JavaRmi">
		<rdfs:subClassOf rdf:resource="&java;JavaAPIPart"/>
		<rdfs:seeAlso rdf:resource="&jdk-1_1;JavaLang"/>
		<rdfs:seeAlso rdf:resource="&jdk-1_1;JavaNet"/>
		<rdfs:seeAlso rdf:resource="&jdk-1_1;JavaIo"/>
		<rdfs:comment xml:lang="en">Java API part implementing the java.rmi package for JDK 1.1</rdfs:comment>
	</owl:Class>
	<owl:Class rdf:about="&jdk-1_1;JavaRmiRegistry">
		<rdfs:subClassOf rdf:resource="&java;JavaAPIPart"/>
		<rdfs:seeAlso rdf:resource="&jdk-1_1;JavaLang"/>
		<rdfs:seeAlso rdf:resource="&jdk-1_1;JavaRmi"/>
		<rdfs:comment xml:lang="en">Java API part implementing the java.rmi.registry package for JDK 1.1</rdfs:comment>
	</owl:Class>
	<owl:Class rdf:about="&jdk-1_1;JavaRmiDgc">
		<rdfs:subClassOf rdf:resource="&java;JavaAPIPart"/>
		<rdfs:seeAlso rdf:resource="&jdk-1_1;JavaLang"/>
		<rdfs:seeAlso rdf:resource="&jdk-1_1;JavaRmi"/>
		<rdfs:seeAlso rdf:resource="&jdk-1_1;JavaIo"/>
		<rdfs:comment xml:lang="en">Java API part implementing the java.rmi.dgc package for JDK 1.1</rdfs:comment>
	</owl:Class>
	<owl:Class rdf:about="&jdk-1_1;JavaRmiServer">
		<rdfs:subClassOf rdf:resource="&java;JavaAPIPart"/>
		<rdfs:seeAlso rdf:resource="&jdk-1_1;JavaLang"/>
		<rdfs:seeAlso rdf:resource="&jdk-1_1;JavaNet"/>
		<rdfs:seeAlso rdf:resource="&jdk-1_1;JavaRmi"/>
		<rdfs:seeAlso rdf:resource="&jdk-1_1;JavaIo"/>
		<rdfs:comment xml:lang="en">Java API part implementing the java.rmi.server package for JDK 1.1</rdfs:comment>
	</owl:Class>
	<owl:Class rdf:about="&jdk-1_1;JavaBeans">
		<owl:equivalentClass rdf:resource="&personaljava-1_1;JavaBeans"/>
		<rdfs:subClassOf rdf:resource="&java;JavaAPIPart"/>
		<rdfs:seeAlso rdf:resource="&jdk-1_1;JavaUtil"/>
		<rdfs:seeAlso rdf:resource="&jdk-1_1;JavaLangReflect"/>
		<rdfs:seeAlso rdf:resource="&jdk-1_1;JavaLang"/>
		<rdfs:seeAlso rdf:resource="&jdk-1_1;JavaIo"/>
		<rdfs:seeAlso rdf:resource="&jdk-1_1;JavaAwt"/>
		<rdfs:comment xml:lang="en">Java API part implementing the java.beans package for JDK 1.1</rdfs:comment>
	</owl:Class>
	<owl:Class rdf:about="&jdk-1_1;JavaLangAPI">
		<owl:equivalentClass rdf:resource="&personaljava-1_1;JavaLangAPI"/>
		<rdfs:subClassOf rdf:resource="&java;JavaAPI"/>
		<rdfs:comment xml:lang="en">JavaLibrary implementing the java.lang package for JDK 1.1</rdfs:comment>
		<rdfs:comment xml:lang="OWLManchester">platform:comprisesInterfacePart some JavaLang</rdfs:comment>
	</owl:Class>
	<owl:Class rdf:about="&jdk-1_1;JavaLangReflectAPI">
		<owl:equivalentClass rdf:resource="&personaljava-1_1;JavaLangReflectAPI"/>
		<rdfs:subClassOf rdf:resource="&java;JavaAPI"/>
		<rdfs:comment xml:lang="en">JavaLibrary implementing the java.lang.reflect package for JDK 1.1</rdfs:comment>
		<rdfs:comment xml:lang="OWLManchester">platform:comprisesInterfacePart some JavaLangReflect</rdfs:comment>
	</owl:Class>
	<owl:Class rdf:about="&jdk-1_1;JavaIoAPI">
		<rdfs:subClassOf rdf:resource="&personaljava-1_1;JavaIoAPI"/>
		<rdfs:comment xml:lang="en">JavaLibrary implementing the java.io package for JDK 1.1</rdfs:comment>
		<rdfs:comment xml:lang="OWLManchester">platform:comprisesInterfacePart some JavaIo</rdfs:comment>
	</owl:Class>
	<owl:Class rdf:about="&jdk-1_1;JavaNetAPI">
		<owl:equivalentClass rdf:resource="&personaljava-1_1;JavaNetAPI"/>
		<rdfs:subClassOf rdf:resource="&java;JavaAPI"/>
		<rdfs:comment xml:lang="en">JavaLibrary implementing the java.net package for JDK 1.1</rdfs:comment>
		<rdfs:comment xml:lang="OWLManchester">platform:comprisesInterfacePart some JavaNet</rdfs:comment>
	</owl:Class>
	<owl:Class rdf:about="&jdk-1_1;JavaUtilAPI">
		<owl:equivalentClass rdf:resource="&personaljava-1_1;JavaUtilAPI"/>
		<rdfs:subClassOf rdf:resource="&java;JavaAPI"/>
		<rdfs:comment xml:lang="en">JavaLibrary implementing the java.util package for JDK 1.1</rdfs:comment>
		<rdfs:comment xml:lang="OWLManchester">platform:comprisesInterfacePart some JavaUtil</rdfs:comment>
	</owl:Class>
	<owl:Class rdf:about="&jdk-1_1;JavaUtilZipAPI">
		<rdfs:subClassOf rdf:resource="&personaljava-1_1;JavaUtilZipAPI"/>
		<rdfs:comment xml:lang="en">JavaLibrary implementing the java.util.zip package for JDK 1.1</rdfs:comment>
		<rdfs:comment xml:lang="OWLManchester">platform:comprisesInterfacePart some JavaUtilZip</rdfs:comment>
	</owl:Class>
	<owl:Class rdf:about="&jdk-1_1;JavaTextAPI">
		<owl:equivalentClass rdf:resource="&personaljava-1_1;JavaTextAPI"/>
		<rdfs:subClassOf rdf:resource="&java;JavaAPI"/>
		<rdfs:comment xml:lang="en">JavaLibrary implementing the java.text package for JDK 1.1</rdfs:comment>
		<rdfs:comment xml:lang="OWLManchester">platform:comprisesInterfacePart some JavaText</rdfs:comment>
	</owl:Class>
	<owl:Class rdf:about="&jdk-1_1;JavaTextResourcesAPI">
		<rdfs:subClassOf rdf:resource="&personaljava-1_1;JavaTextResourcesAPI"/>
		<rdfs:comment xml:lang="en">JavaLibrary implementing the java.text.resources package for JDK 1.1</rdfs:comment>
		<rdfs:comment xml:lang="OWLManchester">platform:comprisesInterfacePart some JavaTextResources</rdfs:comment>
	</owl:Class>
	<owl:Class rdf:about="&jdk-1_1;JavaMathAPI">
		<rdfs:subClassOf rdf:resource="&java;JavaAPI"/>
		<rdfs:comment xml:lang="en">JavaLibrary implementing the java.math package for JDK 1.1</rdfs:comment>
		<rdfs:comment xml:lang="OWLManchester">platform:comprisesInterfacePart some JavaMath</rdfs:comment>
	</owl:Class>
	<owl:Class rdf:about="&jdk-1_1;JavaSecurityAPI">
		<rdfs:subClassOf rdf:resource="&java;JavaAPI"/>
		<rdfs:comment xml:lang="en">JavaLibrary implementing the java.security package for JDK 1.1</rdfs:comment>
		<rdfs:comment xml:lang="OWLManchester">platform:comprisesInterfacePart some JavaSecurity</rdfs:comment>
	</owl:Class>
	<owl:Class rdf:about="&jdk-1_1;JavaSecurityAclAPI">
		<rdfs:subClassOf rdf:resource="&java;JavaAPI"/>
		<rdfs:comment xml:lang="en">JavaLibrary implementing the java.security.acl package for JDK 1.1</rdfs:comment>
		<rdfs:comment xml:lang="OWLManchester">platform:comprisesInterfacePart some JavaSecurityAcl</rdfs:comment>
	</owl:Class>
	<owl:Class rdf:about="&jdk-1_1;JavaSecurityInterfacesAPI">
		<rdfs:subClassOf rdf:resource="&java;JavaAPI"/>
		<rdfs:comment xml:lang="en">JavaLibrary implementing the java.security.interfaces package for JDK 1.1</rdfs:comment>
		<rdfs:comment xml:lang="OWLManchester">platform:comprisesInterfacePart some JavaSecurityInterfaces</rdfs:comment>
	</owl:Class>
	<owl:Class rdf:about="&jdk-1_1;JavaAwtAPI">
		<rdfs:subClassOf rdf:resource="&personaljava-1_1;JavaAwtAPI"/>
		<rdfs:comment xml:lang="en">JavaLibrary implementing the java.awt package for JDK 1.1</rdfs:comment>
		<rdfs:comment xml:lang="OWLManchester">platform:comprisesInterfacePart some JavaAwt</rdfs:comment>
	</owl:Class>
	<owl:Class rdf:about="&jdk-1_1;JavaAwtImageAPI">
		<owl:equivalentClass rdf:resource="&personaljava-1_1;JavaAwtImageAPI"/>
		<rdfs:subClassOf rdf:resource="&java;JavaAPI"/>
		<rdfs:comment xml:lang="en">JavaLibrary implementing the java.awt.image package for JDK 1.1</rdfs:comment>
		<rdfs:comment xml:lang="OWLManchester">platform:comprisesInterfacePart some JavaAwtImage</rdfs:comment>
	</owl:Class>
	<owl:Class rdf:about="&jdk-1_1;JavaAwtDatatransferAPI">
		<owl:equivalentClass rdf:resource="&personaljava-1_1;JavaAwtDatatransferAPI"/>
		<rdfs:subClassOf rdf:resource="&java;JavaAPI"/>
		<rdfs:comment xml:lang="en">JavaLibrary implementing the java.awt.datatransfer package for JDK 1.1</rdfs:comment>
		<rdfs:comment xml:lang="OWLManchester">platform:comprisesInterfacePart some JavaAwtDatatransfer</rdfs:comment>
	</owl:Class>
	<owl:Class rdf:about="&jdk-1_1;JavaAwtEventAPI">
		<owl:equivalentClass rdf:resource="&personaljava-1_1;JavaAwtEventAPI"/>
		<rdfs:subClassOf rdf:resource="&java;JavaAPI"/>
		<rdfs:comment xml:lang="en">JavaLibrary implementing the java.awt.event package for JDK 1.1</rdfs:comment>
		<rdfs:comment xml:lang="OWLManchester">platform:comprisesInterfacePart some JavaAwtEvent</rdfs:comment>
	</owl:Class>
	<owl:Class rdf:about="&jdk-1_1;JavaAppletAPI">
		<owl:equivalentClass rdf:resource="&personaljava-1_1;JavaAppletAPI"/>
		<rdfs:subClassOf rdf:resource="&java;JavaAPI"/>
		<rdfs:comment xml:lang="en">JavaLibrary implementing the java.applet package for JDK 1.1</rdfs:comment>
		<rdfs:comment xml:lang="OWLManchester">platform:comprisesInterfacePart some JavaApplet</rdfs:comment>
	</owl:Class>
	<owl:Class rdf:about="&jdk-1_1;JavaSqlAPI">
		<rdfs:subClassOf rdf:resource="&java;JavaAPI"/>
		<rdfs:comment xml:lang="en">JavaLibrary implementing the java.sql package for JDK 1.1</rdfs:comment>
		<rdfs:comment xml:lang="OWLManchester">platform:comprisesInterfacePart some JavaSql</rdfs:comment>
	</owl:Class>
	<owl:Class rdf:about="&jdk-1_1;JavaRmiAPI">
		<rdfs:subClassOf rdf:resource="&java;JavaAPI"/>
		<rdfs:comment xml:lang="en">JavaLibrary implementing the java.rmi package for JDK 1.1</rdfs:comment>
		<rdfs:comment xml:lang="OWLManchester">platform:comprisesInterfacePart some JavaRmi</rdfs:comment>
	</owl:Class>
	<owl:Class rdf:about="&jdk-1_1;JavaRmiRegistryAPI">
		<rdfs:subClassOf rdf:resource="&java;JavaAPI"/>
		<rdfs:comment xml:lang="en">JavaLibrary implementing the java.rmi.registry package for JDK 1.1</rdfs:comment>
		<rdfs:comment xml:lang="OWLManchester">platform:comprisesInterfacePart some JavaRmiRegistry</rdfs:comment>
	</owl:Class>
	<owl:Class rdf:about="&jdk-1_1;JavaRmiDgcAPI">
		<rdfs:subClassOf rdf:resource="&java;JavaAPI"/>
		<rdfs:comment xml:lang="en">JavaLibrary implementing the java.rmi.dgc package for JDK 1.1</rdfs:comment>
		<rdfs:comment xml:lang="OWLManchester">platform:comprisesInterfacePart some JavaRmiDgc</rdfs:comment>
	</owl:Class>
	<owl:Class rdf:about="&jdk-1_1;JavaRmiServerAPI">
		<rdfs:subClassOf rdf:resource="&java;JavaAPI"/>
		<rdfs:comment xml:lang="en">JavaLibrary implementing the java.rmi.server package for JDK 1.1</rdfs:comment>
		<rdfs:comment xml:lang="OWLManchester">platform:comprisesInterfacePart some JavaRmiServer</rdfs:comment>
	</owl:Class>
	<owl:Class rdf:about="&jdk-1_1;JavaBeansAPI">
		<owl:equivalentClass rdf:resource="&personaljava-1_1;JavaBeansAPI"/>
		<rdfs:subClassOf rdf:resource="&java;JavaAPI"/>
		<rdfs:comment xml:lang="en">JavaLibrary implementing the java.beans package for JDK 1.1</rdfs:comment>
		<rdfs:comment xml:lang="OWLManchester">platform:comprisesInterfacePart some JavaBeans</rdfs:comment>
	</owl:Class>
	<jdk-1_1:JavaLang rdf:about="&jdk-1_1;theJavaLangPart">
	</jdk-1_1:JavaLang>
	<jdk-1_1:JavaLangReflect rdf:about="&jdk-1_1;theJavaLangReflectPart">
	</jdk-1_1:JavaLangReflect>
	<jdk-1_1:JavaIo rdf:about="&jdk-1_1;theJavaIoPart">
	</jdk-1_1:JavaIo>
	<jdk-1_1:JavaNet rdf:about="&jdk-1_1;theJavaNetPart">
	</jdk-1_1:JavaNet>
	<jdk-1_1:JavaUtil rdf:about="&jdk-1_1;theJavaUtilPart">
	</jdk-1_1:JavaUtil>
	<jdk-1_1:JavaUtilZip rdf:about="&jdk-1_1;theJavaUtilZipPart">
	</jdk-1_1:JavaUtilZip>
	<jdk-1_1:JavaText rdf:about="&jdk-1_1;theJavaTextPart">
	</jdk-1_1:JavaText>
	<jdk-1_1:JavaTextResources rdf:about="&jdk-1_1;theJavaTextResourcesPart">
	</jdk-1_1:JavaTextResources>
	<jdk-1_1:JavaMath rdf:about="&jdk-1_1;theJavaMathPart">
	</jdk-1_1:JavaMath>
	<jdk-1_1:JavaSecurity rdf:about="&jdk-1_1;theJavaSecurityPart">
	</jdk-1_1:JavaSecurity>
	<jdk-1_1:JavaSecurityAcl rdf:about="&jdk-1_1;theJavaSecurityAclPart">
	</jdk-1_1:JavaSecurityAcl>
	<jdk-1_1:JavaSecurityInterfaces rdf:about="&jdk-1_1;theJavaSecurityInterfacesPart">
	</jdk-1_1:JavaSecurityInterfaces>
	<jdk-1_1:JavaAwt rdf:about="&jdk-1_1;theJavaAwtPart">
	</jdk-1_1:JavaAwt>
	<jdk-1_1:JavaAwtImage rdf:about="&jdk-1_1;theJavaAwtImagePart">
	</jdk-1_1:JavaAwtImage>
	<jdk-1_1:JavaAwtDatatransfer rdf:about="&jdk-1_1;theJavaAwtDatatransferPart">
	</jdk-1_1:JavaAwtDatatransfer>
	<jdk-1_1:JavaAwtEvent rdf:about="&jdk-1_1;theJavaAwtEventPart">
	</jdk-1_1:JavaAwtEvent>
	<jdk-1_1:JavaApplet rdf:about="&jdk-1_1;theJavaAppletPart">
	</jdk-1_1:JavaApplet>
	<jdk-1_1:JavaSql rdf:about="&jdk-1_1;theJavaSqlPart">
	</jdk-1_1:JavaSql>
	<jdk-1_1:JavaRmi rdf:about="&jdk-1_1;theJavaRmiPart">
	</jdk-1_1:JavaRmi>
	<jdk-1_1:JavaRmiRegistry rdf:about="&jdk-1_1;theJavaRmiRegistryPart">
	</jdk-1_1:JavaRmiRegistry>
	<jdk-1_1:JavaRmiDgc rdf:about="&jdk-1_1;theJavaRmiDgcPart">
	</jdk-1_1:JavaRmiDgc>
	<jdk-1_1:JavaRmiServer rdf:about="&jdk-1_1;theJavaRmiServerPart">
	</jdk-1_1:JavaRmiServer>
	<jdk-1_1:JavaBeans rdf:about="&jdk-1_1;theJavaBeansPart">
	</jdk-1_1:JavaBeans>
	<owl:Class rdf:about="&jdk-1_1;JavaLangClassLibrary">
		<owl:equivalentClass rdf:resource="&personaljava-1_1;JavaLangClassLibrary"/>
		<rdfs:subClassOf rdf:resource="&java;JavaClassLibrary"/>
		<rdfs:comment xml:lang="en">JavaLibrary implementing the java.lang package for JDK 1.1</rdfs:comment>
		<rdfs:comment xml:lang="OWLManchester">platform:implementsInterface some JavaLangAPI</rdfs:comment>
	</owl:Class>
	<owl:Class rdf:about="&jdk-1_1;JavaLangReflectClassLibrary">
		<owl:equivalentClass rdf:resource="&personaljava-1_1;JavaLangReflectClassLibrary"/>
		<rdfs:subClassOf rdf:resource="&java;JavaClassLibrary"/>
		<rdfs:comment xml:lang="en">JavaLibrary implementing the java.lang.reflect package for JDK 1.1</rdfs:comment>
		<rdfs:comment xml:lang="OWLManchester">platform:implementsInterface some JavaLangReflectAPI</rdfs:comment>
	</owl:Class>
	<owl:Class rdf:about="&jdk-1_1;JavaIoClassLibrary">
		<rdfs:subClassOf rdf:resource="&personaljava-1_1;JavaIoClassLibrary"/>
		<rdfs:comment xml:lang="en">JavaLibrary implementing the java.io package for JDK 1.1</rdfs:comment>
		<rdfs:comment xml:lang="OWLManchester">platform:implementsInterface some JavaIoAPI</rdfs:comment>
	</owl:Class>
	<owl:Class rdf:about="&jdk-1_1;JavaNetClassLibrary">
		<owl:equivalentClass rdf:resource="&personaljava-1_1;JavaNetClassLibrary"/>
		<rdfs:subClassOf rdf:resource="&java;JavaClassLibrary"/>
		<rdfs:comment xml:lang="en">JavaLibrary implementing the java.net package for JDK 1.1</rdfs:comment>
		<rdfs:comment xml:lang="OWLManchester">platform:implementsInterface some JavaNetAPI</rdfs:comment>
	</owl:Class>
	<owl:Class rdf:about="&jdk-1_1;JavaUtilClassLibrary">
		<owl:equivalentClass rdf:resource="&personaljava-1_1;JavaUtilClassLibrary"/>
		<rdfs:subClassOf rdf:resource="&java;JavaClassLibrary"/>
		<rdfs:comment xml:lang="en">JavaLibrary implementing the java.util package for JDK 1.1</rdfs:comment>
		<rdfs:comment xml:lang="OWLManchester">platform:implementsInterface some JavaUtilAPI</rdfs:comment>
	</owl:Class>
	<owl:Class rdf:about="&jdk-1_1;JavaUtilZipClassLibrary">
		<rdfs:subClassOf rdf:resource="&personaljava-1_1;JavaUtilZipClassLibrary"/>
		<rdfs:comment xml:lang="en">JavaLibrary implementing the java.util.zip package for JDK 1.1</rdfs:comment>
		<rdfs:comment xml:lang="OWLManchester">platform:implementsInterface some JavaUtilZipAPI</rdfs:comment>
	</owl:Class>
	<owl:Class rdf:about="&jdk-1_1;JavaTextClassLibrary">
		<owl:equivalentClass rdf:resource="&personaljava-1_1;JavaTextClassLibrary"/>
		<rdfs:subClassOf rdf:resource="&java;JavaClassLibrary"/>
		<rdfs:comment xml:lang="en">JavaLibrary implementing the java.text package for JDK 1.1</rdfs:comment>
		<rdfs:comment xml:lang="OWLManchester">platform:implementsInterface some JavaTextAPI</rdfs:comment>
	</owl:Class>
	<owl:Class rdf:about="&jdk-1_1;JavaTextResourcesClassLibrary">
		<rdfs:subClassOf rdf:resource="&personaljava-1_1;JavaTextResourcesClassLibrary"/>
		<rdfs:comment xml:lang="en">JavaLibrary implementing the java.text.resources package for JDK 1.1</rdfs:comment>
		<rdfs:comment xml:lang="OWLManchester">platform:implementsInterface some JavaTextResourcesAPI</rdfs:comment>
	</owl:Class>
	<owl:Class rdf:about="&jdk-1_1;JavaMathClassLibrary">
		<rdfs:subClassOf rdf:resource="&java;JavaClassLibrary"/>
		<rdfs:comment xml:lang="en">JavaLibrary implementing the java.math package for JDK 1.1</rdfs:comment>
		<rdfs:comment xml:lang="OWLManchester">platform:implementsInterface some JavaMathAPI</rdfs:comment>
	</owl:Class>
	<owl:Class rdf:about="&jdk-1_1;JavaSecurityClassLibrary">
		<rdfs:subClassOf rdf:resource="&java;JavaClassLibrary"/>
		<rdfs:comment xml:lang="en">JavaLibrary implementing the java.security package for JDK 1.1</rdfs:comment>
		<rdfs:comment xml:lang="OWLManchester">platform:implementsInterface some JavaSecurityAPI</rdfs:comment>
	</owl:Class>
	<owl:Class rdf:about="&jdk-1_1;JavaSecurityAclClassLibrary">
		<rdfs:subClassOf rdf:resource="&java;JavaClassLibrary"/>
		<rdfs:comment xml:lang="en">JavaLibrary implementing the java.security.acl package for JDK 1.1</rdfs:comment>
		<rdfs:comment xml:lang="OWLManchester">platform:implementsInterface some JavaSecurityAclAPI</rdfs:comment>
	</owl:Class>
	<owl:Class rdf:about="&jdk-1_1;JavaSecurityInterfacesClassLibrary">
		<rdfs:subClassOf rdf:resource="&java;JavaClassLibrary"/>
		<rdfs:comment xml:lang="en">JavaLibrary implementing the java.security.interfaces package for JDK 1.1</rdfs:comment>
		<rdfs:comment xml:lang="OWLManchester">platform:implementsInterface some JavaSecurityInterfacesAPI</rdfs:comment>
	</owl:Class>
	<owl:Class rdf:about="&jdk-1_1;JavaAwtClassLibrary">
		<rdfs:subClassOf rdf:resource="&personaljava-1_1;JavaAwtClassLibrary"/>
		<rdfs:comment xml:lang="en">JavaLibrary implementing the java.awt package for JDK 1.1</rdfs:comment>
		<rdfs:comment xml:lang="OWLManchester">platform:implementsInterface some JavaAwtAPI</rdfs:comment>
	</owl:Class>
	<owl:Class rdf:about="&jdk-1_1;JavaAwtImageClassLibrary">
		<owl:equivalentClass rdf:resource="&personaljava-1_1;JavaAwtImageClassLibrary"/>
		<rdfs:subClassOf rdf:resource="&java;JavaClassLibrary"/>
		<rdfs:comment xml:lang="en">JavaLibrary implementing the java.awt.image package for JDK 1.1</rdfs:comment>
		<rdfs:comment xml:lang="OWLManchester">platform:implementsInterface some JavaAwtImageAPI</rdfs:comment>
	</owl:Class>
	<owl:Class rdf:about="&jdk-1_1;JavaAwtDatatransferClassLibrary">
		<owl:equivalentClass rdf:resource="&personaljava-1_1;JavaAwtDatatransferClassLibrary"/>
		<rdfs:subClassOf rdf:resource="&java;JavaClassLibrary"/>
		<rdfs:comment xml:lang="en">JavaLibrary implementing the java.awt.datatransfer package for JDK 1.1</rdfs:comment>
		<rdfs:comment xml:lang="OWLManchester">platform:implementsInterface some JavaAwtDatatransferAPI</rdfs:comment>
	</owl:Class>
	<owl:Class rdf:about="&jdk-1_1;JavaAwtEventClassLibrary">
		<owl:equivalentClass rdf:resource="&personaljava-1_1;JavaAwtEventClassLibrary"/>
		<rdfs:subClassOf rdf:resource="&java;JavaClassLibrary"/>
		<rdfs:comment xml:lang="en">JavaLibrary implementing the java.awt.event package for JDK 1.1</rdfs:comment>
		<rdfs:comment xml:lang="OWLManchester">platform:implementsInterface some JavaAwtEventAPI</rdfs:comment>
	</owl:Class>
	<owl:Class rdf:about="&jdk-1_1;JavaAppletClassLibrary">
		<owl:equivalentClass rdf:resource="&personaljava-1_1;JavaAppletClassLibrary"/>
		<rdfs:subClassOf rdf:resource="&java;JavaClassLibrary"/>
		<rdfs:comment xml:lang="en">JavaLibrary implementing the java.applet package for JDK 1.1</rdfs:comment>
		<rdfs:comment xml:lang="OWLManchester">platform:implementsInterface some JavaAppletAPI</rdfs:comment>
	</owl:Class>
	<owl:Class rdf:about="&jdk-1_1;JavaSqlClassLibrary">
		<rdfs:subClassOf rdf:resource="&java;JavaClassLibrary"/>
		<rdfs:comment xml:lang="en">JavaLibrary implementing the java.sql package for JDK 1.1</rdfs:comment>
		<rdfs:comment xml:lang="OWLManchester">platform:implementsInterface some JavaSqlAPI</rdfs:comment>
	</owl:Class>
	<owl:Class rdf:about="&jdk-1_1;JavaRmiClassLibrary">
		<rdfs:subClassOf rdf:resource="&java;JavaClassLibrary"/>
		<rdfs:comment xml:lang="en">JavaLibrary implementing the java.rmi package for JDK 1.1</rdfs:comment>
		<rdfs:comment xml:lang="OWLManchester">platform:implementsInterface some JavaRmiAPI</rdfs:comment>
	</owl:Class>
	<owl:Class rdf:about="&jdk-1_1;JavaRmiRegistryClassLibrary">
		<rdfs:subClassOf rdf:resource="&java;JavaClassLibrary"/>
		<rdfs:comment xml:lang="en">JavaLibrary implementing the java.rmi.registry package for JDK 1.1</rdfs:comment>
		<rdfs:comment xml:lang="OWLManchester">platform:implementsInterface some JavaRmiRegistryAPI</rdfs:comment>
	</owl:Class>
	<owl:Class rdf:about="&jdk-1_1;JavaRmiDgcClassLibrary">
		<rdfs:subClassOf rdf:resource="&java;JavaClassLibrary"/>
		<rdfs:comment xml:lang="en">JavaLibrary implementing the java.rmi.dgc package for JDK 1.1</rdfs:comment>
		<rdfs:comment xml:lang="OWLManchester">platform:implementsInterface some JavaRmiDgcAPI</rdfs:comment>
	</owl:Class>
	<owl:Class rdf:about="&jdk-1_1;JavaRmiServerClassLibrary">
		<rdfs:subClassOf rdf:resource="&java;JavaClassLibrary"/>
		<rdfs:comment xml:lang="en">JavaLibrary implementing the java.rmi.server package for JDK 1.1</rdfs:comment>
		<rdfs:comment xml:lang="OWLManchester">platform:implementsInterface some JavaRmiServerAPI</rdfs:comment>
	</owl:Class>
	<owl:Class rdf:about="&jdk-1_1;JavaBeansClassLibrary">
		<owl:equivalentClass rdf:resource="&personaljava-1_1;JavaBeansClassLibrary"/>
		<rdfs:subClassOf rdf:resource="&java;JavaClassLibrary"/>
		<rdfs:comment xml:lang="en">JavaLibrary implementing the java.beans package for JDK 1.1</rdfs:comment>
		<rdfs:comment xml:lang="OWLManchester">platform:implementsInterface some JavaBeansAPI</rdfs:comment>
	</owl:Class>
</rdf:RDF>
