<?xml version="1.0" encoding="ISO-8859-1"?>
<!DOCTYPE rdf:RDF [
	<!ENTITY java "http://localhost/~dennis/Java.owl#">
	<!ENTITY j2me-midp-2_0 "http://ssel.vub.ac.be/platformkit/j2me-midp-2_0#">
	<!ENTITY units "http://localhost/~dennis/Units.owl#">
	<!ENTITY platform "http://localhost/~dennis/Platform.owl#">
	<!ENTITY xsd "http://www.w3.org/2001/XMLSchema#">
	<!ENTITY j2me-midp-1_0 "http://ssel.vub.ac.be/platformkit/j2me-midp-1_0#">
	<!ENTITY rdf "http://www.w3.org/1999/02/22-rdf-syntax-ns#">
	<!ENTITY rdfs "http://www.w3.org/2000/01/rdf-schema#">
	<!ENTITY owl "http://www.w3.org/2002/07/owl#">
]>
<rdf:RDF
	 xmlns:java="&java;"
	 xmlns:j2me-midp-2_0="&j2me-midp-2_0;"
	 xmlns:units="&units;"
	 xmlns:platform="&platform;"
	 xmlns:xsd="&xsd;"
	 xmlns:j2me-midp-1_0="&j2me-midp-1_0;"
	 xmlns:rdf="&rdf;"
	 xmlns:rdfs="&rdfs;"
	 xmlns:owl="&owl;"
>

	<owl:Ontology rdf:about="http://ssel.vub.ac.be/platformkit/j2me-midp-2_0#">
		<owl:imports rdf:resource="http://localhost/~dennis/Platform.owl"/>
		<owl:imports rdf:resource="http://localhost/~dennis/Java.owl"/>
		<owl:imports rdf:resource="http://ssel.vub.ac.be/platformkit/j2me-midp-1_0#"/>
		<rdfs:comment xml:lang="en">Generated by $Id: UML2ToPackageAPIOntology.atl 7380 2007-11-08 09:49:02Z dwagelaa $ and $Id: UML2ToAPIOntology.atl 7380 2007-11-08 09:49:02Z dwagelaa $ and $Id:UML2Comparison.atl 7084 2007-07-10 13:19:05Z dwagelaa $</rdfs:comment>
		<rdfs:label xml:lang="en">j2me-midp-2_0</rdfs:label>
	</owl:Ontology>
	<owl:Class rdf:about="&j2me-midp-2_0;J2me-midp-2_0ClassLibrary">
		<rdfs:subClassOf rdf:resource="&j2me-midp-2_0;JavaUtilLibrary"/>
		<rdfs:subClassOf rdf:resource="&j2me-midp-2_0;JavaLangLibrary"/>
		<rdfs:subClassOf rdf:resource="&j2me-midp-2_0;JavaLangRefLibrary"/>
		<rdfs:subClassOf rdf:resource="&j2me-midp-2_0;JavaIoLibrary"/>
		<rdfs:subClassOf rdf:resource="&j2me-midp-2_0;JavaxMicroeditionIoLibrary"/>
		<rdfs:subClassOf rdf:resource="&j2me-midp-2_0;JavaxMicroeditionPkiLibrary"/>
		<rdfs:subClassOf rdf:resource="&j2me-midp-2_0;JavaxMicroeditionLcduiLibrary"/>
		<rdfs:subClassOf rdf:resource="&j2me-midp-2_0;JavaxMicroeditionLcduiGameLibrary"/>
		<rdfs:subClassOf rdf:resource="&j2me-midp-2_0;JavaxMicroeditionMidletLibrary"/>
		<rdfs:subClassOf rdf:resource="&j2me-midp-2_0;JavaxMicroeditionRmsLibrary"/>
		<rdfs:subClassOf rdf:resource="&j2me-midp-2_0;JavaxMicroeditionMediaLibrary"/>
		<rdfs:subClassOf rdf:resource="&j2me-midp-2_0;JavaxMicroeditionMediaProtocolLibrary"/>
		<rdfs:subClassOf rdf:resource="&j2me-midp-2_0;JavaxMicroeditionMediaControlLibrary"/>
		<rdfs:comment xml:lang="en">JavaLibrary implementing the entire API for j2me-midp-2_0</rdfs:comment>
	</owl:Class>
	<owl:Class rdf:about="&j2me-midp-2_0;J2me-midp-2_0">
		<rdfs:subClassOf rdf:resource="&java;JRE"/>
		<rdfs:subClassOf>
			<owl:Restriction>
				<owl:onProperty rdf:resource="&java;providesBuiltinJavaLibrary"/>
				<owl:someValuesFrom rdf:resource="&j2me-midp-2_0;J2me-midp-2_0ClassLibrary"/>
			</owl:Restriction>
		</rdfs:subClassOf>
		<rdfs:comment xml:lang="en">j2me-midp-2_0 Java Runtime Environment</rdfs:comment>
	</owl:Class>
	<owl:Class rdf:about="&j2me-midp-2_0;JavaUtilLibrary">
		<rdfs:subClassOf rdf:resource="&j2me-midp-1_0;JavaUtilLibrary"/>
		<rdfs:seeAlso rdf:resource="&j2me-midp-2_0;JavaLangLibrary"/>
		<rdfs:comment xml:lang="en">JavaLibrary implementing the java.util package for j2me-midp-2_0</rdfs:comment>
	</owl:Class>
	<owl:Class rdf:about="&j2me-midp-2_0;JavaLangLibrary">
		<rdfs:subClassOf rdf:resource="&j2me-midp-1_0;JavaLangLibrary"/>
		<rdfs:seeAlso rdf:resource="&j2me-midp-2_0;JavaIoLibrary"/>
		<rdfs:comment xml:lang="en">JavaLibrary implementing the java.lang package for j2me-midp-2_0</rdfs:comment>
	</owl:Class>
	<owl:Class rdf:about="&j2me-midp-2_0;JavaLangRefLibrary">
		<rdfs:subClassOf rdf:resource="&java;JavaLibrary"/>
		<rdfs:seeAlso rdf:resource="&j2me-midp-2_0;JavaLangLibrary"/>
		<rdfs:comment xml:lang="en">JavaLibrary implementing the java.lang.ref package for j2me-midp-2_0</rdfs:comment>
	</owl:Class>
	<owl:Class rdf:about="&j2me-midp-2_0;JavaIoLibrary">
		<rdfs:subClassOf rdf:resource="&j2me-midp-1_0;JavaIoLibrary"/>
		<rdfs:seeAlso rdf:resource="&j2me-midp-2_0;JavaLangLibrary"/>
		<rdfs:comment xml:lang="en">JavaLibrary implementing the java.io package for j2me-midp-2_0</rdfs:comment>
	</owl:Class>
	<owl:Class rdf:about="&j2me-midp-2_0;JavaxMicroeditionIoLibrary">
		<rdfs:subClassOf rdf:resource="&j2me-midp-1_0;JavaxMicroeditionIoLibrary"/>
		<rdfs:seeAlso rdf:resource="&j2me-midp-2_0;JavaLangLibrary"/>
		<rdfs:seeAlso rdf:resource="&j2me-midp-2_0;JavaIoLibrary"/>
		<rdfs:seeAlso rdf:resource="&j2me-midp-2_0;JavaxMicroeditionPkiLibrary"/>
		<rdfs:comment xml:lang="en">JavaLibrary implementing the javax.microedition.io package for j2me-midp-2_0</rdfs:comment>
	</owl:Class>
	<owl:Class rdf:about="&j2me-midp-2_0;JavaxMicroeditionPkiLibrary">
		<rdfs:subClassOf rdf:resource="&java;JavaLibrary"/>
		<rdfs:seeAlso rdf:resource="&j2me-midp-2_0;JavaLangLibrary"/>
		<rdfs:seeAlso rdf:resource="&j2me-midp-2_0;JavaIoLibrary"/>
		<rdfs:comment xml:lang="en">JavaLibrary implementing the javax.microedition.pki package for j2me-midp-2_0</rdfs:comment>
	</owl:Class>
	<owl:Class rdf:about="&j2me-midp-2_0;JavaxMicroeditionLcduiLibrary">
		<rdfs:subClassOf rdf:resource="&j2me-midp-1_0;JavaxMicroeditionLcduiLibrary"/>
		<rdfs:seeAlso rdf:resource="&j2me-midp-2_0;JavaxMicroeditionMidletLibrary"/>
		<rdfs:seeAlso rdf:resource="&j2me-midp-2_0;JavaLangLibrary"/>
		<rdfs:seeAlso rdf:resource="&j2me-midp-2_0;JavaUtilLibrary"/>
		<rdfs:seeAlso rdf:resource="&j2me-midp-2_0;JavaIoLibrary"/>
		<rdfs:comment xml:lang="en">JavaLibrary implementing the javax.microedition.lcdui package for j2me-midp-2_0</rdfs:comment>
	</owl:Class>
	<owl:Class rdf:about="&j2me-midp-2_0;JavaxMicroeditionLcduiGameLibrary">
		<rdfs:subClassOf rdf:resource="&java;JavaLibrary"/>
		<rdfs:seeAlso rdf:resource="&j2me-midp-2_0;JavaLangLibrary"/>
		<rdfs:seeAlso rdf:resource="&j2me-midp-2_0;JavaxMicroeditionLcduiLibrary"/>
		<rdfs:comment xml:lang="en">JavaLibrary implementing the javax.microedition.lcdui.game package for j2me-midp-2_0</rdfs:comment>
	</owl:Class>
	<owl:Class rdf:about="&j2me-midp-2_0;JavaxMicroeditionMidletLibrary">
		<rdfs:subClassOf rdf:resource="&j2me-midp-1_0;JavaxMicroeditionMidletLibrary"/>
		<rdfs:seeAlso rdf:resource="&j2me-midp-2_0;JavaLangLibrary"/>
		<rdfs:comment xml:lang="en">JavaLibrary implementing the javax.microedition.midlet package for j2me-midp-2_0</rdfs:comment>
	</owl:Class>
	<owl:Class rdf:about="&j2me-midp-2_0;JavaxMicroeditionRmsLibrary">
		<rdfs:subClassOf rdf:resource="&j2me-midp-1_0;JavaxMicroeditionRmsLibrary"/>
		<rdfs:seeAlso rdf:resource="&j2me-midp-2_0;JavaLangLibrary"/>
		<rdfs:comment xml:lang="en">JavaLibrary implementing the javax.microedition.rms package for j2me-midp-2_0</rdfs:comment>
	</owl:Class>
	<owl:Class rdf:about="&j2me-midp-2_0;JavaxMicroeditionMediaLibrary">
		<rdfs:subClassOf rdf:resource="&java;JavaLibrary"/>
		<rdfs:seeAlso rdf:resource="&j2me-midp-2_0;JavaLangLibrary"/>
		<rdfs:seeAlso rdf:resource="&j2me-midp-2_0;JavaxMicroeditionMediaProtocolLibrary"/>
		<rdfs:seeAlso rdf:resource="&j2me-midp-2_0;JavaIoLibrary"/>
		<rdfs:comment xml:lang="en">JavaLibrary implementing the javax.microedition.media package for j2me-midp-2_0</rdfs:comment>
	</owl:Class>
	<owl:Class rdf:about="&j2me-midp-2_0;JavaxMicroeditionMediaProtocolLibrary">
		<rdfs:subClassOf rdf:resource="&java;JavaLibrary"/>
		<rdfs:seeAlso rdf:resource="&j2me-midp-2_0;JavaxMicroeditionMediaLibrary"/>
		<rdfs:seeAlso rdf:resource="&j2me-midp-2_0;JavaLangLibrary"/>
		<rdfs:comment xml:lang="en">JavaLibrary implementing the javax.microedition.media.protocol package for j2me-midp-2_0</rdfs:comment>
	</owl:Class>
	<owl:Class rdf:about="&j2me-midp-2_0;JavaxMicroeditionMediaControlLibrary">
		<rdfs:subClassOf rdf:resource="&java;JavaLibrary"/>
		<rdfs:seeAlso rdf:resource="&j2me-midp-2_0;JavaxMicroeditionMediaLibrary"/>
		<rdfs:comment xml:lang="en">JavaLibrary implementing the javax.microedition.media.control package for j2me-midp-2_0</rdfs:comment>
	</owl:Class>
</rdf:RDF>
