<?xml version="1.0" encoding="ISO-8859-1"?>
<!DOCTYPE rdf:RDF [
	<!ENTITY xsd "http://www.w3.org/2001/XMLSchema#">
	<!ENTITY java "http://localhost/~dennis/platformkit/2010_1/java.owl#">
	<!ENTITY j2se-1_4 "http://soft.vub.ac.be/platformkit/2010/1/j2se-1_4.owl#">
	<!ENTITY isa "http://localhost/~dennis/platformkit/2010_1/isa.owl#">
	<!ENTITY ns_19 "http://localhost/~dennis/platformkit/2010_1/">
	<!ENTITY platform "http://localhost/~dennis/platformkit/2010_1/platform.owl#">
	<!ENTITY j2se-5_0 "http://soft.vub.ac.be/platformkit/2010/1/j2se-5_0.owl#">
	<!ENTITY rdf "http://www.w3.org/1999/02/22-rdf-syntax-ns#">
	<!ENTITY rdfs "http://www.w3.org/2000/01/rdf-schema#">
	<!ENTITY owl "http://www.w3.org/2002/07/owl#">
]>
<rdf:RDF
	 xmlns:xsd="&xsd;"
	 xmlns:java="&java;"
	 xmlns:j2se-1_4="&j2se-1_4;"
	 xmlns:isa="&isa;"
	 xmlns:ns_19="&ns_19;"
	 xmlns:platform="&platform;"
	 xmlns:j2se-5_0="&j2se-5_0;"
	 xmlns:rdf="&rdf;"
	 xmlns:rdfs="&rdfs;"
	 xmlns:owl="&owl;"
>

	<owl:Ontology rdf:about="http://soft.vub.ac.be/platformkit/2010/1/j2se-5_0.owl#">
		<owl:versionInfo>$Id: UML2ToPackageAPIOntology.atl 8082 2010-03-18 21:11:00Z dwagelaa $</owl:versionInfo>
		<owl:imports rdf:resource="http://localhost/~dennis/platformkit/2010_1/platform.owl"/>
		<owl:imports rdf:resource="http://localhost/~dennis/platformkit/2010_1/java.owl"/>
		<owl:imports rdf:resource="http://soft.vub.ac.be/platformkit/2010/1/j2se-1_4.owl#"/>
		<owl:imports rdf:resource="http://localhost/~dennis/platformkit/2010_1/isa.owl"/>
		<rdfs:comment xml:lang="en">Generated by [UML2ToSimplifiedPackageAPIOntology.atl 8080 2010-03-18 10:46:40Z dwagelaa], [UML2ToPackageAPIOntology.atl 8082 2010-03-18 21:11:00Z dwagelaa], [UML2ToAPIOntology.atl 8082 2010-03-18 21:11:00Z dwagelaa], and [UML2Comparison.atl 8082 2010-03-18 21:11:00Z dwagelaa]</rdfs:comment>
		<rdfs:comment>Dennis Wagelaar &lt;dennis.wagelaar@vub.ac.be&gt;</rdfs:comment>
		<rdfs:comment xml:lang="en">&#169; 2010, Vrije Universiteit Brussel. All rights reserved.</rdfs:comment>
		<rdfs:label xml:lang="en">J2SE 5.0</rdfs:label>
	</owl:Ontology>
	<owl:Class rdf:about="&j2se-5_0;J2SE5_0API">
		<rdfs:subClassOf rdf:resource="&j2se-5_0;JavaxCryptoAPI"/>
		<rdfs:subClassOf rdf:resource="&j2se-5_0;JavaxCryptoInterfacesAPI"/>
		<rdfs:subClassOf rdf:resource="&j2se-5_0;JavaxCryptoSpecAPI"/>
		<rdfs:subClassOf rdf:resource="&j2se-5_0;JavaxNetAPI"/>
		<rdfs:subClassOf rdf:resource="&j2se-5_0;JavaxNetSslAPI"/>
		<rdfs:subClassOf rdf:resource="&j2se-5_0;JavaxSecurityCertAPI"/>
		<rdfs:subClassOf rdf:resource="&j2se-5_0;JavaxSecurityAuthAPI"/>
		<rdfs:subClassOf rdf:resource="&j2se-5_0;JavaxSecurityAuthCallbackAPI"/>
		<rdfs:subClassOf rdf:resource="&j2se-5_0;JavaxSecurityAuthX500API"/>
		<rdfs:subClassOf rdf:resource="&j2se-5_0;JavaxSecurityAuthKerberosAPI"/>
		<rdfs:subClassOf rdf:resource="&j2se-5_0;JavaxSecurityAuthLoginAPI"/>
		<rdfs:subClassOf rdf:resource="&j2se-5_0;JavaxSecurityAuthSpiAPI"/>
		<rdfs:subClassOf rdf:resource="&j2se-5_0;JavaxSecuritySaslAPI"/>
		<rdfs:subClassOf rdf:resource="&j2se-5_0;JavaxAccessibilityAPI"/>
		<rdfs:subClassOf rdf:resource="&j2se-5_0;JavaxSwingAPI"/>
		<rdfs:subClassOf rdf:resource="&j2se-5_0;JavaxSwingTextAPI"/>
		<rdfs:subClassOf rdf:resource="&j2se-5_0;JavaxSwingTextHtmlAPI"/>
		<rdfs:subClassOf rdf:resource="&j2se-5_0;JavaxSwingTextHtmlParserAPI"/>
		<rdfs:subClassOf rdf:resource="&j2se-5_0;JavaxSwingTextRtfAPI"/>
		<rdfs:subClassOf rdf:resource="&j2se-5_0;JavaxSwingEventAPI"/>
		<rdfs:subClassOf rdf:resource="&j2se-5_0;JavaxSwingColorchooserAPI"/>
		<rdfs:subClassOf rdf:resource="&j2se-5_0;JavaxSwingPlafAPI"/>
		<rdfs:subClassOf rdf:resource="&j2se-5_0;JavaxSwingPlafBasicAPI"/>
		<rdfs:subClassOf rdf:resource="&j2se-5_0;JavaxSwingPlafMetalAPI"/>
		<rdfs:subClassOf rdf:resource="&j2se-5_0;JavaxSwingPlafMultiAPI"/>
		<rdfs:subClassOf rdf:resource="&j2se-5_0;JavaxSwingPlafSynthAPI"/>
		<rdfs:subClassOf rdf:resource="&j2se-5_0;JavaxSwingTreeAPI"/>
		<rdfs:subClassOf rdf:resource="&j2se-5_0;JavaxSwingBorderAPI"/>
		<rdfs:subClassOf rdf:resource="&j2se-5_0;JavaxSwingFilechooserAPI"/>
		<rdfs:subClassOf rdf:resource="&j2se-5_0;JavaxSwingTableAPI"/>
		<rdfs:subClassOf rdf:resource="&j2se-5_0;JavaxSwingUndoAPI"/>
		<rdfs:subClassOf rdf:resource="&j2se-5_0;JavaxManagementAPI"/>
		<rdfs:subClassOf rdf:resource="&j2se-5_0;JavaxManagementOpenmbeanAPI"/>
		<rdfs:subClassOf rdf:resource="&j2se-5_0;JavaxManagementLoadingAPI"/>
		<rdfs:subClassOf rdf:resource="&j2se-5_0;JavaxManagementModelmbeanAPI"/>
		<rdfs:subClassOf rdf:resource="&j2se-5_0;JavaxManagementMonitorAPI"/>
		<rdfs:subClassOf rdf:resource="&j2se-5_0;JavaxManagementRelationAPI"/>
		<rdfs:subClassOf rdf:resource="&j2se-5_0;JavaxManagementRemoteAPI"/>
		<rdfs:subClassOf rdf:resource="&j2se-5_0;JavaxManagementRemoteRmiAPI"/>
		<rdfs:subClassOf rdf:resource="&j2se-5_0;JavaxManagementTimerAPI"/>
		<rdfs:subClassOf rdf:resource="&j2se-5_0;JavaxActivityAPI"/>
		<rdfs:subClassOf rdf:resource="&j2se-5_0;JavaxImageioAPI"/>
		<rdfs:subClassOf rdf:resource="&j2se-5_0;JavaxImageioMetadataAPI"/>
		<rdfs:subClassOf rdf:resource="&j2se-5_0;JavaxImageioEventAPI"/>
		<rdfs:subClassOf rdf:resource="&j2se-5_0;JavaxImageioPluginsBmpAPI"/>
		<rdfs:subClassOf rdf:resource="&j2se-5_0;JavaxImageioPluginsJpegAPI"/>
		<rdfs:subClassOf rdf:resource="&j2se-5_0;JavaxImageioStreamAPI"/>
		<rdfs:subClassOf rdf:resource="&j2se-5_0;JavaxImageioSpiAPI"/>
		<rdfs:subClassOf rdf:resource="&j2se-5_0;JavaxNamingAPI"/>
		<rdfs:subClassOf rdf:resource="&j2se-5_0;JavaxNamingDirectoryAPI"/>
		<rdfs:subClassOf rdf:resource="&j2se-5_0;JavaxNamingEventAPI"/>
		<rdfs:subClassOf rdf:resource="&j2se-5_0;JavaxNamingLdapAPI"/>
		<rdfs:subClassOf rdf:resource="&j2se-5_0;JavaxNamingSpiAPI"/>
		<rdfs:subClassOf rdf:resource="&j2se-5_0;JavaxPrintAPI"/>
		<rdfs:subClassOf rdf:resource="&j2se-5_0;JavaxPrintAttributeAPI"/>
		<rdfs:subClassOf rdf:resource="&j2se-5_0;JavaxPrintAttributeStandardAPI"/>
		<rdfs:subClassOf rdf:resource="&j2se-5_0;JavaxPrintEventAPI"/>
		<rdfs:subClassOf rdf:resource="&j2se-5_0;JavaxRmiAPI"/>
		<rdfs:subClassOf rdf:resource="&j2se-5_0;JavaxRmiCORBAAPI"/>
		<rdfs:subClassOf rdf:resource="&j2se-5_0;JavaxRmiSslAPI"/>
		<rdfs:subClassOf rdf:resource="&j2se-5_0;JavaxSoundMidiAPI"/>
		<rdfs:subClassOf rdf:resource="&j2se-5_0;JavaxSoundMidiSpiAPI"/>
		<rdfs:subClassOf rdf:resource="&j2se-5_0;JavaxSoundSampledAPI"/>
		<rdfs:subClassOf rdf:resource="&j2se-5_0;JavaxSoundSampledSpiAPI"/>
		<rdfs:subClassOf rdf:resource="&j2se-5_0;JavaxSqlAPI"/>
		<rdfs:subClassOf rdf:resource="&j2se-5_0;JavaxSqlRowsetAPI"/>
		<rdfs:subClassOf rdf:resource="&j2se-5_0;JavaxSqlRowsetSpiAPI"/>
		<rdfs:subClassOf rdf:resource="&j2se-5_0;JavaxSqlRowsetSerialAPI"/>
		<rdfs:subClassOf rdf:resource="&j2se-5_0;JavaxTransactionAPI"/>
		<rdfs:subClassOf rdf:resource="&j2se-5_0;JavaxTransactionXaAPI"/>
		<rdfs:subClassOf rdf:resource="&j2se-5_0;JavaxXmlAPI"/>
		<rdfs:subClassOf rdf:resource="&j2se-5_0;JavaxXmlDatatypeAPI"/>
		<rdfs:subClassOf rdf:resource="&j2se-5_0;JavaxXmlNamespaceAPI"/>
		<rdfs:subClassOf rdf:resource="&j2se-5_0;JavaxXmlTransformAPI"/>
		<rdfs:subClassOf rdf:resource="&j2se-5_0;JavaxXmlTransformDomAPI"/>
		<rdfs:subClassOf rdf:resource="&j2se-5_0;JavaxXmlTransformSaxAPI"/>
		<rdfs:subClassOf rdf:resource="&j2se-5_0;JavaxXmlTransformStreamAPI"/>
		<rdfs:subClassOf rdf:resource="&j2se-5_0;JavaxXmlValidationAPI"/>
		<rdfs:subClassOf rdf:resource="&j2se-5_0;JavaxXmlXpathAPI"/>
		<rdfs:subClassOf rdf:resource="&j2se-5_0;JavaxXmlParsersAPI"/>
		<rdfs:subClassOf rdf:resource="&j2se-5_0;JavaLangAPI"/>
		<rdfs:subClassOf rdf:resource="&j2se-5_0;JavaLangReflectAPI"/>
		<rdfs:subClassOf rdf:resource="&j2se-5_0;JavaLangAnnotationAPI"/>
		<rdfs:subClassOf rdf:resource="&j2se-5_0;JavaLangInstrumentAPI"/>
		<rdfs:subClassOf rdf:resource="&j2se-5_0;JavaLangManagementAPI"/>
		<rdfs:subClassOf rdf:resource="&j2se-5_0;JavaLangRefAPI"/>
		<rdfs:subClassOf rdf:resource="&j2se-5_0;JavaSecurityAPI"/>
		<rdfs:subClassOf rdf:resource="&j2se-5_0;JavaSecuritySpecAPI"/>
		<rdfs:subClassOf rdf:resource="&j2se-5_0;JavaSecurityCertAPI"/>
		<rdfs:subClassOf rdf:resource="&j2se-5_0;JavaSecurityAclAPI"/>
		<rdfs:subClassOf rdf:resource="&j2se-5_0;JavaSecurityInterfacesAPI"/>
		<rdfs:subClassOf rdf:resource="&j2se-5_0;JavaMathAPI"/>
		<rdfs:subClassOf rdf:resource="&j2se-5_0;JavaNioAPI"/>
		<rdfs:subClassOf rdf:resource="&j2se-5_0;JavaNioChannelsAPI"/>
		<rdfs:subClassOf rdf:resource="&j2se-5_0;JavaNioChannelsSpiAPI"/>
		<rdfs:subClassOf rdf:resource="&j2se-5_0;JavaNioCharsetAPI"/>
		<rdfs:subClassOf rdf:resource="&j2se-5_0;JavaNioCharsetSpiAPI"/>
		<rdfs:subClassOf rdf:resource="&j2se-5_0;JavaIoAPI"/>
		<rdfs:subClassOf rdf:resource="&j2se-5_0;JavaNetAPI"/>
		<rdfs:subClassOf rdf:resource="&j2se-5_0;JavaUtilAPI"/>
		<rdfs:subClassOf rdf:resource="&j2se-5_0;JavaUtilRegexAPI"/>
		<rdfs:subClassOf rdf:resource="&j2se-5_0;JavaUtilConcurrentAPI"/>
		<rdfs:subClassOf rdf:resource="&j2se-5_0;JavaUtilConcurrentAtomicAPI"/>
		<rdfs:subClassOf rdf:resource="&j2se-5_0;JavaUtilConcurrentLocksAPI"/>
		<rdfs:subClassOf rdf:resource="&j2se-5_0;JavaUtilJarAPI"/>
		<rdfs:subClassOf rdf:resource="&j2se-5_0;JavaUtilZipAPI"/>
		<rdfs:subClassOf rdf:resource="&j2se-5_0;JavaUtilLoggingAPI"/>
		<rdfs:subClassOf rdf:resource="&j2se-5_0;JavaUtilPrefsAPI"/>
		<rdfs:subClassOf rdf:resource="&j2se-5_0;JavaAppletAPI"/>
		<rdfs:subClassOf rdf:resource="&j2se-5_0;JavaAwtAPI"/>
		<rdfs:subClassOf rdf:resource="&j2se-5_0;JavaAwtEventAPI"/>
		<rdfs:subClassOf rdf:resource="&j2se-5_0;JavaAwtImageAPI"/>
		<rdfs:subClassOf rdf:resource="&j2se-5_0;JavaAwtImageRenderableAPI"/>
		<rdfs:subClassOf rdf:resource="&j2se-5_0;JavaAwtGeomAPI"/>
		<rdfs:subClassOf rdf:resource="&j2se-5_0;JavaAwtImAPI"/>
		<rdfs:subClassOf rdf:resource="&j2se-5_0;JavaAwtImSpiAPI"/>
		<rdfs:subClassOf rdf:resource="&j2se-5_0;JavaAwtColorAPI"/>
		<rdfs:subClassOf rdf:resource="&j2se-5_0;JavaAwtDatatransferAPI"/>
		<rdfs:subClassOf rdf:resource="&j2se-5_0;JavaAwtDndAPI"/>
		<rdfs:subClassOf rdf:resource="&j2se-5_0;JavaAwtFontAPI"/>
		<rdfs:subClassOf rdf:resource="&j2se-5_0;JavaAwtPrintAPI"/>
		<rdfs:subClassOf rdf:resource="&j2se-5_0;JavaTextAPI"/>
		<rdfs:subClassOf rdf:resource="&j2se-5_0;JavaBeansAPI"/>
		<rdfs:subClassOf rdf:resource="&j2se-5_0;JavaBeansBeancontextAPI"/>
		<rdfs:subClassOf rdf:resource="&j2se-5_0;JavaRmiAPI"/>
		<rdfs:subClassOf rdf:resource="&j2se-5_0;JavaRmiActivationAPI"/>
		<rdfs:subClassOf rdf:resource="&j2se-5_0;JavaRmiServerAPI"/>
		<rdfs:subClassOf rdf:resource="&j2se-5_0;JavaRmiDgcAPI"/>
		<rdfs:subClassOf rdf:resource="&j2se-5_0;JavaRmiRegistryAPI"/>
		<rdfs:subClassOf rdf:resource="&j2se-5_0;JavaSqlAPI"/>
		<rdfs:subClassOf rdf:resource="&j2se-5_0;OrgW3cDomAPI"/>
		<rdfs:subClassOf rdf:resource="&j2se-5_0;OrgW3cDomLsAPI"/>
		<rdfs:subClassOf rdf:resource="&j2se-5_0;OrgW3cDomBootstrapAPI"/>
		<rdfs:subClassOf rdf:resource="&j2se-5_0;OrgW3cDomCssAPI"/>
		<rdfs:subClassOf rdf:resource="&j2se-5_0;OrgW3cDomStylesheetsAPI"/>
		<rdfs:subClassOf rdf:resource="&j2se-5_0;OrgW3cDomViewsAPI"/>
		<rdfs:subClassOf rdf:resource="&j2se-5_0;OrgW3cDomEventsAPI"/>
		<rdfs:subClassOf rdf:resource="&j2se-5_0;OrgW3cDomHtmlAPI"/>
		<rdfs:subClassOf rdf:resource="&j2se-5_0;OrgW3cDomTraversalAPI"/>
		<rdfs:subClassOf rdf:resource="&j2se-5_0;OrgW3cDomRangesAPI"/>
		<rdfs:subClassOf rdf:resource="&j2se-5_0;OrgOmgCORBA_2_3API"/>
		<rdfs:subClassOf rdf:resource="&j2se-5_0;OrgOmgCORBA_2_3PortableAPI"/>
		<rdfs:subClassOf rdf:resource="&j2se-5_0;OrgOmgCORBAAPI"/>
		<rdfs:subClassOf rdf:resource="&j2se-5_0;OrgOmgCORBAPortableAPI"/>
		<rdfs:subClassOf rdf:resource="&j2se-5_0;OrgOmgCORBADynAnyPackageAPI"/>
		<rdfs:subClassOf rdf:resource="&j2se-5_0;OrgOmgCORBAORBPackageAPI"/>
		<rdfs:subClassOf rdf:resource="&j2se-5_0;OrgOmgCORBATypeCodePackageAPI"/>
		<rdfs:subClassOf rdf:resource="&j2se-5_0;OrgOmgSendingContextAPI"/>
		<rdfs:subClassOf rdf:resource="&j2se-5_0;OrgOmgCosNamingAPI"/>
		<rdfs:subClassOf rdf:resource="&j2se-5_0;OrgOmgCosNamingNamingContextExtPackageAPI"/>
		<rdfs:subClassOf rdf:resource="&j2se-5_0;OrgOmgCosNamingNamingContextPackageAPI"/>
		<rdfs:subClassOf rdf:resource="&j2se-5_0;OrgOmgPortableServerAPI"/>
		<rdfs:subClassOf rdf:resource="&j2se-5_0;OrgOmgPortableServerCurrentPackageAPI"/>
		<rdfs:subClassOf rdf:resource="&j2se-5_0;OrgOmgPortableServerPOAManagerPackageAPI"/>
		<rdfs:subClassOf rdf:resource="&j2se-5_0;OrgOmgPortableServerPOAPackageAPI"/>
		<rdfs:subClassOf rdf:resource="&j2se-5_0;OrgOmgPortableServerPortableAPI"/>
		<rdfs:subClassOf rdf:resource="&j2se-5_0;OrgOmgPortableServerServantLocatorPackageAPI"/>
		<rdfs:subClassOf rdf:resource="&j2se-5_0;OrgOmgDynamicAPI"/>
		<rdfs:subClassOf rdf:resource="&j2se-5_0;OrgOmgDynamicAnyAPI"/>
		<rdfs:subClassOf rdf:resource="&j2se-5_0;OrgOmgDynamicAnyDynAnyFactoryPackageAPI"/>
		<rdfs:subClassOf rdf:resource="&j2se-5_0;OrgOmgDynamicAnyDynAnyPackageAPI"/>
		<rdfs:subClassOf rdf:resource="&j2se-5_0;OrgOmgIOPAPI"/>
		<rdfs:subClassOf rdf:resource="&j2se-5_0;OrgOmgIOPCodecFactoryPackageAPI"/>
		<rdfs:subClassOf rdf:resource="&j2se-5_0;OrgOmgIOPCodecPackageAPI"/>
		<rdfs:subClassOf rdf:resource="&j2se-5_0;OrgOmgMessagingAPI"/>
		<rdfs:subClassOf rdf:resource="&j2se-5_0;OrgOmgPortableInterceptorAPI"/>
		<rdfs:subClassOf rdf:resource="&j2se-5_0;OrgOmgPortableInterceptorORBInitInfoPackageAPI"/>
		<rdfs:subClassOf rdf:resource="&j2se-5_0;OrgOmgStubJavaRmiAPI"/>
		<rdfs:subClassOf rdf:resource="&j2se-5_0;OrgOmgStubJavaxManagementRemoteRmiAPI"/>
		<rdfs:subClassOf rdf:resource="&j2se-5_0;OrgXmlSaxAPI"/>
		<rdfs:subClassOf rdf:resource="&j2se-5_0;OrgXmlSaxExtAPI"/>
		<rdfs:subClassOf rdf:resource="&j2se-5_0;OrgXmlSaxHelpersAPI"/>
		<rdfs:subClassOf rdf:resource="&j2se-5_0;OrgIetfJgssAPI"/>
		<rdfs:comment xml:lang="en">J2SE 5.0 API</rdfs:comment>
		<rdfs:comment xml:lang="OWLManchester">platform:comprisesInterfacePart some JavaxCrypto and platform:comprisesInterfacePart some JavaxCryptoInterfaces and platform:comprisesInterfacePart some JavaxCryptoSpec and platform:comprisesInterfacePart some JavaxNet and platform:comprisesInterfacePart some JavaxNetSsl and platform:comprisesInterfacePart some JavaxSecurityCert and platform:comprisesInterfacePart some JavaxSecurityAuth and platform:comprisesInterfacePart some JavaxSecurityAuthCallback and platform:comprisesInterfacePart some JavaxSecurityAuthX500 and platform:comprisesInterfacePart some JavaxSecurityAuthKerberos and platform:comprisesInterfacePart some JavaxSecurityAuthLogin and platform:comprisesInterfacePart some JavaxSecurityAuthSpi and platform:comprisesInterfacePart some JavaxSecuritySasl and platform:comprisesInterfacePart some JavaxAccessibility and platform:comprisesInterfacePart some JavaxSwing and platform:comprisesInterfacePart some JavaxSwingText and platform:comprisesInterfacePart some JavaxSwingTextHtml and platform:comprisesInterfacePart some JavaxSwingTextHtmlParser and platform:comprisesInterfacePart some JavaxSwingTextRtf and platform:comprisesInterfacePart some JavaxSwingEvent and platform:comprisesInterfacePart some JavaxSwingColorchooser and platform:comprisesInterfacePart some JavaxSwingPlaf and platform:comprisesInterfacePart some JavaxSwingPlafBasic and platform:comprisesInterfacePart some JavaxSwingPlafMetal and platform:comprisesInterfacePart some JavaxSwingPlafMulti and platform:comprisesInterfacePart some JavaxSwingPlafSynth and platform:comprisesInterfacePart some JavaxSwingTree and platform:comprisesInterfacePart some JavaxSwingBorder and platform:comprisesInterfacePart some JavaxSwingFilechooser and platform:comprisesInterfacePart some JavaxSwingTable and platform:comprisesInterfacePart some JavaxSwingUndo and platform:comprisesInterfacePart some JavaxManagement and platform:comprisesInterfacePart some JavaxManagementOpenmbean and platform:comprisesInterfacePart some JavaxManagementLoading and platform:comprisesInterfacePart some JavaxManagementModelmbean and platform:comprisesInterfacePart some JavaxManagementMonitor and platform:comprisesInterfacePart some JavaxManagementRelation and platform:comprisesInterfacePart some JavaxManagementRemote and platform:comprisesInterfacePart some JavaxManagementRemoteRmi and platform:comprisesInterfacePart some JavaxManagementTimer and platform:comprisesInterfacePart some JavaxActivity and platform:comprisesInterfacePart some JavaxImageio and platform:comprisesInterfacePart some JavaxImageioMetadata and platform:comprisesInterfacePart some JavaxImageioEvent and platform:comprisesInterfacePart some JavaxImageioPluginsBmp and platform:comprisesInterfacePart some JavaxImageioPluginsJpeg and platform:comprisesInterfacePart some JavaxImageioStream and platform:comprisesInterfacePart some JavaxImageioSpi and platform:comprisesInterfacePart some JavaxNaming and platform:comprisesInterfacePart some JavaxNamingDirectory and platform:comprisesInterfacePart some JavaxNamingEvent and platform:comprisesInterfacePart some JavaxNamingLdap and platform:comprisesInterfacePart some JavaxNamingSpi and platform:comprisesInterfacePart some JavaxPrint and platform:comprisesInterfacePart some JavaxPrintAttribute and platform:comprisesInterfacePart some JavaxPrintAttributeStandard and platform:comprisesInterfacePart some JavaxPrintEvent and platform:comprisesInterfacePart some JavaxRmi and platform:comprisesInterfacePart some JavaxRmiCORBA and platform:comprisesInterfacePart some JavaxRmiSsl and platform:comprisesInterfacePart some JavaxSoundMidi and platform:comprisesInterfacePart some JavaxSoundMidiSpi and platform:comprisesInterfacePart some JavaxSoundSampled and platform:comprisesInterfacePart some JavaxSoundSampledSpi and platform:comprisesInterfacePart some JavaxSql and platform:comprisesInterfacePart some JavaxSqlRowset and platform:comprisesInterfacePart some JavaxSqlRowsetSpi and platform:comprisesInterfacePart some JavaxSqlRowsetSerial and platform:comprisesInterfacePart some JavaxTransaction and platform:comprisesInterfacePart some JavaxTransactionXa and platform:comprisesInterfacePart some JavaxXml and platform:comprisesInterfacePart some JavaxXmlDatatype and platform:comprisesInterfacePart some JavaxXmlNamespace and platform:comprisesInterfacePart some JavaxXmlTransform and platform:comprisesInterfacePart some JavaxXmlTransformDom and platform:comprisesInterfacePart some JavaxXmlTransformSax and platform:comprisesInterfacePart some JavaxXmlTransformStream and platform:comprisesInterfacePart some JavaxXmlValidation and platform:comprisesInterfacePart some JavaxXmlXpath and platform:comprisesInterfacePart some JavaxXmlParsers and platform:comprisesInterfacePart some JavaLang and platform:comprisesInterfacePart some JavaLangReflect and platform:comprisesInterfacePart some JavaLangAnnotation and platform:comprisesInterfacePart some JavaLangInstrument and platform:comprisesInterfacePart some JavaLangManagement and platform:comprisesInterfacePart some JavaLangRef and platform:comprisesInterfacePart some JavaSecurity and platform:comprisesInterfacePart some JavaSecuritySpec and platform:comprisesInterfacePart some JavaSecurityCert and platform:comprisesInterfacePart some JavaSecurityAcl and platform:comprisesInterfacePart some JavaSecurityInterfaces and platform:comprisesInterfacePart some JavaMath and platform:comprisesInterfacePart some JavaNio and platform:comprisesInterfacePart some JavaNioChannels and platform:comprisesInterfacePart some JavaNioChannelsSpi and platform:comprisesInterfacePart some JavaNioCharset and platform:comprisesInterfacePart some JavaNioCharsetSpi and platform:comprisesInterfacePart some JavaIo and platform:comprisesInterfacePart some JavaNet and platform:comprisesInterfacePart some JavaUtil and platform:comprisesInterfacePart some JavaUtilRegex and platform:comprisesInterfacePart some JavaUtilConcurrent and platform:comprisesInterfacePart some JavaUtilConcurrentAtomic and platform:comprisesInterfacePart some JavaUtilConcurrentLocks and platform:comprisesInterfacePart some JavaUtilJar and platform:comprisesInterfacePart some JavaUtilZip and platform:comprisesInterfacePart some JavaUtilLogging and platform:comprisesInterfacePart some JavaUtilPrefs and platform:comprisesInterfacePart some JavaApplet and platform:comprisesInterfacePart some JavaAwt and platform:comprisesInterfacePart some JavaAwtEvent and platform:comprisesInterfacePart some JavaAwtImage and platform:comprisesInterfacePart some JavaAwtImageRenderable and platform:comprisesInterfacePart some JavaAwtGeom and platform:comprisesInterfacePart some JavaAwtIm and platform:comprisesInterfacePart some JavaAwtImSpi and platform:comprisesInterfacePart some JavaAwtColor and platform:comprisesInterfacePart some JavaAwtDatatransfer and platform:comprisesInterfacePart some JavaAwtDnd and platform:comprisesInterfacePart some JavaAwtFont and platform:comprisesInterfacePart some JavaAwtPrint and platform:comprisesInterfacePart some JavaText and platform:comprisesInterfacePart some JavaBeans and platform:comprisesInterfacePart some JavaBeansBeancontext and platform:comprisesInterfacePart some JavaRmi and platform:comprisesInterfacePart some JavaRmiActivation and platform:comprisesInterfacePart some JavaRmiServer and platform:comprisesInterfacePart some JavaRmiDgc and platform:comprisesInterfacePart some JavaRmiRegistry and platform:comprisesInterfacePart some JavaSql and platform:comprisesInterfacePart some OrgW3cDom and platform:comprisesInterfacePart some OrgW3cDomLs and platform:comprisesInterfacePart some OrgW3cDomBootstrap and platform:comprisesInterfacePart some OrgW3cDomCss and platform:comprisesInterfacePart some OrgW3cDomStylesheets and platform:comprisesInterfacePart some OrgW3cDomViews and platform:comprisesInterfacePart some OrgW3cDomEvents and platform:comprisesInterfacePart some OrgW3cDomHtml and platform:comprisesInterfacePart some OrgW3cDomTraversal and platform:comprisesInterfacePart some OrgW3cDomRanges and platform:comprisesInterfacePart some OrgOmgCORBA_2_3 and platform:comprisesInterfacePart some OrgOmgCORBA_2_3Portable and platform:comprisesInterfacePart some OrgOmgCORBA and platform:comprisesInterfacePart some OrgOmgCORBAPortable and platform:comprisesInterfacePart some OrgOmgCORBADynAnyPackage and platform:comprisesInterfacePart some OrgOmgCORBAORBPackage and platform:comprisesInterfacePart some OrgOmgCORBATypeCodePackage and platform:comprisesInterfacePart some OrgOmgSendingContext and platform:comprisesInterfacePart some OrgOmgCosNaming and platform:comprisesInterfacePart some OrgOmgCosNamingNamingContextExtPackage and platform:comprisesInterfacePart some OrgOmgCosNamingNamingContextPackage and platform:comprisesInterfacePart some OrgOmgPortableServer and platform:comprisesInterfacePart some OrgOmgPortableServerCurrentPackage and platform:comprisesInterfacePart some OrgOmgPortableServerPOAManagerPackage and platform:comprisesInterfacePart some OrgOmgPortableServerPOAPackage and platform:comprisesInterfacePart some OrgOmgPortableServerPortable and platform:comprisesInterfacePart some OrgOmgPortableServerServantLocatorPackage and platform:comprisesInterfacePart some OrgOmgDynamic and platform:comprisesInterfacePart some OrgOmgDynamicAny and platform:comprisesInterfacePart some OrgOmgDynamicAnyDynAnyFactoryPackage and platform:comprisesInterfacePart some OrgOmgDynamicAnyDynAnyPackage and platform:comprisesInterfacePart some OrgOmgIOP and platform:comprisesInterfacePart some OrgOmgIOPCodecFactoryPackage and platform:comprisesInterfacePart some OrgOmgIOPCodecPackage and platform:comprisesInterfacePart some OrgOmgMessaging and platform:comprisesInterfacePart some OrgOmgPortableInterceptor and platform:comprisesInterfacePart some OrgOmgPortableInterceptorORBInitInfoPackage and platform:comprisesInterfacePart some OrgOmgStubJavaRmi and platform:comprisesInterfacePart some OrgOmgStubJavaxManagementRemoteRmi and platform:comprisesInterfacePart some OrgXmlSax and platform:comprisesInterfacePart some OrgXmlSaxExt and platform:comprisesInterfacePart some OrgXmlSaxHelpers and platform:comprisesInterfacePart some OrgIetfJgss</rdfs:comment>
	</owl:Class>
	<owl:Class rdf:about="&j2se-5_0;J2SE5_0ClassLibrary">
		<rdfs:subClassOf rdf:resource="&j2se-5_0;JavaxCryptoClassLibrary"/>
		<rdfs:subClassOf rdf:resource="&j2se-5_0;JavaxCryptoInterfacesClassLibrary"/>
		<rdfs:subClassOf rdf:resource="&j2se-5_0;JavaxCryptoSpecClassLibrary"/>
		<rdfs:subClassOf rdf:resource="&j2se-5_0;JavaxNetClassLibrary"/>
		<rdfs:subClassOf rdf:resource="&j2se-5_0;JavaxNetSslClassLibrary"/>
		<rdfs:subClassOf rdf:resource="&j2se-5_0;JavaxSecurityCertClassLibrary"/>
		<rdfs:subClassOf rdf:resource="&j2se-5_0;JavaxSecurityAuthClassLibrary"/>
		<rdfs:subClassOf rdf:resource="&j2se-5_0;JavaxSecurityAuthCallbackClassLibrary"/>
		<rdfs:subClassOf rdf:resource="&j2se-5_0;JavaxSecurityAuthX500ClassLibrary"/>
		<rdfs:subClassOf rdf:resource="&j2se-5_0;JavaxSecurityAuthKerberosClassLibrary"/>
		<rdfs:subClassOf rdf:resource="&j2se-5_0;JavaxSecurityAuthLoginClassLibrary"/>
		<rdfs:subClassOf rdf:resource="&j2se-5_0;JavaxSecurityAuthSpiClassLibrary"/>
		<rdfs:subClassOf rdf:resource="&j2se-5_0;JavaxSecuritySaslClassLibrary"/>
		<rdfs:subClassOf rdf:resource="&j2se-5_0;JavaxAccessibilityClassLibrary"/>
		<rdfs:subClassOf rdf:resource="&j2se-5_0;JavaxSwingClassLibrary"/>
		<rdfs:subClassOf rdf:resource="&j2se-5_0;JavaxSwingTextClassLibrary"/>
		<rdfs:subClassOf rdf:resource="&j2se-5_0;JavaxSwingTextHtmlClassLibrary"/>
		<rdfs:subClassOf rdf:resource="&j2se-5_0;JavaxSwingTextHtmlParserClassLibrary"/>
		<rdfs:subClassOf rdf:resource="&j2se-5_0;JavaxSwingTextRtfClassLibrary"/>
		<rdfs:subClassOf rdf:resource="&j2se-5_0;JavaxSwingEventClassLibrary"/>
		<rdfs:subClassOf rdf:resource="&j2se-5_0;JavaxSwingColorchooserClassLibrary"/>
		<rdfs:subClassOf rdf:resource="&j2se-5_0;JavaxSwingPlafClassLibrary"/>
		<rdfs:subClassOf rdf:resource="&j2se-5_0;JavaxSwingPlafBasicClassLibrary"/>
		<rdfs:subClassOf rdf:resource="&j2se-5_0;JavaxSwingPlafMetalClassLibrary"/>
		<rdfs:subClassOf rdf:resource="&j2se-5_0;JavaxSwingPlafMultiClassLibrary"/>
		<rdfs:subClassOf rdf:resource="&j2se-5_0;JavaxSwingPlafSynthClassLibrary"/>
		<rdfs:subClassOf rdf:resource="&j2se-5_0;JavaxSwingTreeClassLibrary"/>
		<rdfs:subClassOf rdf:resource="&j2se-5_0;JavaxSwingBorderClassLibrary"/>
		<rdfs:subClassOf rdf:resource="&j2se-5_0;JavaxSwingFilechooserClassLibrary"/>
		<rdfs:subClassOf rdf:resource="&j2se-5_0;JavaxSwingTableClassLibrary"/>
		<rdfs:subClassOf rdf:resource="&j2se-5_0;JavaxSwingUndoClassLibrary"/>
		<rdfs:subClassOf rdf:resource="&j2se-5_0;JavaxManagementClassLibrary"/>
		<rdfs:subClassOf rdf:resource="&j2se-5_0;JavaxManagementOpenmbeanClassLibrary"/>
		<rdfs:subClassOf rdf:resource="&j2se-5_0;JavaxManagementLoadingClassLibrary"/>
		<rdfs:subClassOf rdf:resource="&j2se-5_0;JavaxManagementModelmbeanClassLibrary"/>
		<rdfs:subClassOf rdf:resource="&j2se-5_0;JavaxManagementMonitorClassLibrary"/>
		<rdfs:subClassOf rdf:resource="&j2se-5_0;JavaxManagementRelationClassLibrary"/>
		<rdfs:subClassOf rdf:resource="&j2se-5_0;JavaxManagementRemoteClassLibrary"/>
		<rdfs:subClassOf rdf:resource="&j2se-5_0;JavaxManagementRemoteRmiClassLibrary"/>
		<rdfs:subClassOf rdf:resource="&j2se-5_0;JavaxManagementTimerClassLibrary"/>
		<rdfs:subClassOf rdf:resource="&j2se-5_0;JavaxActivityClassLibrary"/>
		<rdfs:subClassOf rdf:resource="&j2se-5_0;JavaxImageioClassLibrary"/>
		<rdfs:subClassOf rdf:resource="&j2se-5_0;JavaxImageioMetadataClassLibrary"/>
		<rdfs:subClassOf rdf:resource="&j2se-5_0;JavaxImageioEventClassLibrary"/>
		<rdfs:subClassOf rdf:resource="&j2se-5_0;JavaxImageioPluginsBmpClassLibrary"/>
		<rdfs:subClassOf rdf:resource="&j2se-5_0;JavaxImageioPluginsJpegClassLibrary"/>
		<rdfs:subClassOf rdf:resource="&j2se-5_0;JavaxImageioStreamClassLibrary"/>
		<rdfs:subClassOf rdf:resource="&j2se-5_0;JavaxImageioSpiClassLibrary"/>
		<rdfs:subClassOf rdf:resource="&j2se-5_0;JavaxNamingClassLibrary"/>
		<rdfs:subClassOf rdf:resource="&j2se-5_0;JavaxNamingDirectoryClassLibrary"/>
		<rdfs:subClassOf rdf:resource="&j2se-5_0;JavaxNamingEventClassLibrary"/>
		<rdfs:subClassOf rdf:resource="&j2se-5_0;JavaxNamingLdapClassLibrary"/>
		<rdfs:subClassOf rdf:resource="&j2se-5_0;JavaxNamingSpiClassLibrary"/>
		<rdfs:subClassOf rdf:resource="&j2se-5_0;JavaxPrintClassLibrary"/>
		<rdfs:subClassOf rdf:resource="&j2se-5_0;JavaxPrintAttributeClassLibrary"/>
		<rdfs:subClassOf rdf:resource="&j2se-5_0;JavaxPrintAttributeStandardClassLibrary"/>
		<rdfs:subClassOf rdf:resource="&j2se-5_0;JavaxPrintEventClassLibrary"/>
		<rdfs:subClassOf rdf:resource="&j2se-5_0;JavaxRmiClassLibrary"/>
		<rdfs:subClassOf rdf:resource="&j2se-5_0;JavaxRmiCORBAClassLibrary"/>
		<rdfs:subClassOf rdf:resource="&j2se-5_0;JavaxRmiSslClassLibrary"/>
		<rdfs:subClassOf rdf:resource="&j2se-5_0;JavaxSoundMidiClassLibrary"/>
		<rdfs:subClassOf rdf:resource="&j2se-5_0;JavaxSoundMidiSpiClassLibrary"/>
		<rdfs:subClassOf rdf:resource="&j2se-5_0;JavaxSoundSampledClassLibrary"/>
		<rdfs:subClassOf rdf:resource="&j2se-5_0;JavaxSoundSampledSpiClassLibrary"/>
		<rdfs:subClassOf rdf:resource="&j2se-5_0;JavaxSqlClassLibrary"/>
		<rdfs:subClassOf rdf:resource="&j2se-5_0;JavaxSqlRowsetClassLibrary"/>
		<rdfs:subClassOf rdf:resource="&j2se-5_0;JavaxSqlRowsetSpiClassLibrary"/>
		<rdfs:subClassOf rdf:resource="&j2se-5_0;JavaxSqlRowsetSerialClassLibrary"/>
		<rdfs:subClassOf rdf:resource="&j2se-5_0;JavaxTransactionClassLibrary"/>
		<rdfs:subClassOf rdf:resource="&j2se-5_0;JavaxTransactionXaClassLibrary"/>
		<rdfs:subClassOf rdf:resource="&j2se-5_0;JavaxXmlClassLibrary"/>
		<rdfs:subClassOf rdf:resource="&j2se-5_0;JavaxXmlDatatypeClassLibrary"/>
		<rdfs:subClassOf rdf:resource="&j2se-5_0;JavaxXmlNamespaceClassLibrary"/>
		<rdfs:subClassOf rdf:resource="&j2se-5_0;JavaxXmlTransformClassLibrary"/>
		<rdfs:subClassOf rdf:resource="&j2se-5_0;JavaxXmlTransformDomClassLibrary"/>
		<rdfs:subClassOf rdf:resource="&j2se-5_0;JavaxXmlTransformSaxClassLibrary"/>
		<rdfs:subClassOf rdf:resource="&j2se-5_0;JavaxXmlTransformStreamClassLibrary"/>
		<rdfs:subClassOf rdf:resource="&j2se-5_0;JavaxXmlValidationClassLibrary"/>
		<rdfs:subClassOf rdf:resource="&j2se-5_0;JavaxXmlXpathClassLibrary"/>
		<rdfs:subClassOf rdf:resource="&j2se-5_0;JavaxXmlParsersClassLibrary"/>
		<rdfs:subClassOf rdf:resource="&j2se-5_0;JavaLangClassLibrary"/>
		<rdfs:subClassOf rdf:resource="&j2se-5_0;JavaLangReflectClassLibrary"/>
		<rdfs:subClassOf rdf:resource="&j2se-5_0;JavaLangAnnotationClassLibrary"/>
		<rdfs:subClassOf rdf:resource="&j2se-5_0;JavaLangInstrumentClassLibrary"/>
		<rdfs:subClassOf rdf:resource="&j2se-5_0;JavaLangManagementClassLibrary"/>
		<rdfs:subClassOf rdf:resource="&j2se-5_0;JavaLangRefClassLibrary"/>
		<rdfs:subClassOf rdf:resource="&j2se-5_0;JavaSecurityClassLibrary"/>
		<rdfs:subClassOf rdf:resource="&j2se-5_0;JavaSecuritySpecClassLibrary"/>
		<rdfs:subClassOf rdf:resource="&j2se-5_0;JavaSecurityCertClassLibrary"/>
		<rdfs:subClassOf rdf:resource="&j2se-5_0;JavaSecurityAclClassLibrary"/>
		<rdfs:subClassOf rdf:resource="&j2se-5_0;JavaSecurityInterfacesClassLibrary"/>
		<rdfs:subClassOf rdf:resource="&j2se-5_0;JavaMathClassLibrary"/>
		<rdfs:subClassOf rdf:resource="&j2se-5_0;JavaNioClassLibrary"/>
		<rdfs:subClassOf rdf:resource="&j2se-5_0;JavaNioChannelsClassLibrary"/>
		<rdfs:subClassOf rdf:resource="&j2se-5_0;JavaNioChannelsSpiClassLibrary"/>
		<rdfs:subClassOf rdf:resource="&j2se-5_0;JavaNioCharsetClassLibrary"/>
		<rdfs:subClassOf rdf:resource="&j2se-5_0;JavaNioCharsetSpiClassLibrary"/>
		<rdfs:subClassOf rdf:resource="&j2se-5_0;JavaIoClassLibrary"/>
		<rdfs:subClassOf rdf:resource="&j2se-5_0;JavaNetClassLibrary"/>
		<rdfs:subClassOf rdf:resource="&j2se-5_0;JavaUtilClassLibrary"/>
		<rdfs:subClassOf rdf:resource="&j2se-5_0;JavaUtilRegexClassLibrary"/>
		<rdfs:subClassOf rdf:resource="&j2se-5_0;JavaUtilConcurrentClassLibrary"/>
		<rdfs:subClassOf rdf:resource="&j2se-5_0;JavaUtilConcurrentAtomicClassLibrary"/>
		<rdfs:subClassOf rdf:resource="&j2se-5_0;JavaUtilConcurrentLocksClassLibrary"/>
		<rdfs:subClassOf rdf:resource="&j2se-5_0;JavaUtilJarClassLibrary"/>
		<rdfs:subClassOf rdf:resource="&j2se-5_0;JavaUtilZipClassLibrary"/>
		<rdfs:subClassOf rdf:resource="&j2se-5_0;JavaUtilLoggingClassLibrary"/>
		<rdfs:subClassOf rdf:resource="&j2se-5_0;JavaUtilPrefsClassLibrary"/>
		<rdfs:subClassOf rdf:resource="&j2se-5_0;JavaAppletClassLibrary"/>
		<rdfs:subClassOf rdf:resource="&j2se-5_0;JavaAwtClassLibrary"/>
		<rdfs:subClassOf rdf:resource="&j2se-5_0;JavaAwtEventClassLibrary"/>
		<rdfs:subClassOf rdf:resource="&j2se-5_0;JavaAwtImageClassLibrary"/>
		<rdfs:subClassOf rdf:resource="&j2se-5_0;JavaAwtImageRenderableClassLibrary"/>
		<rdfs:subClassOf rdf:resource="&j2se-5_0;JavaAwtGeomClassLibrary"/>
		<rdfs:subClassOf rdf:resource="&j2se-5_0;JavaAwtImClassLibrary"/>
		<rdfs:subClassOf rdf:resource="&j2se-5_0;JavaAwtImSpiClassLibrary"/>
		<rdfs:subClassOf rdf:resource="&j2se-5_0;JavaAwtColorClassLibrary"/>
		<rdfs:subClassOf rdf:resource="&j2se-5_0;JavaAwtDatatransferClassLibrary"/>
		<rdfs:subClassOf rdf:resource="&j2se-5_0;JavaAwtDndClassLibrary"/>
		<rdfs:subClassOf rdf:resource="&j2se-5_0;JavaAwtFontClassLibrary"/>
		<rdfs:subClassOf rdf:resource="&j2se-5_0;JavaAwtPrintClassLibrary"/>
		<rdfs:subClassOf rdf:resource="&j2se-5_0;JavaTextClassLibrary"/>
		<rdfs:subClassOf rdf:resource="&j2se-5_0;JavaBeansClassLibrary"/>
		<rdfs:subClassOf rdf:resource="&j2se-5_0;JavaBeansBeancontextClassLibrary"/>
		<rdfs:subClassOf rdf:resource="&j2se-5_0;JavaRmiClassLibrary"/>
		<rdfs:subClassOf rdf:resource="&j2se-5_0;JavaRmiActivationClassLibrary"/>
		<rdfs:subClassOf rdf:resource="&j2se-5_0;JavaRmiServerClassLibrary"/>
		<rdfs:subClassOf rdf:resource="&j2se-5_0;JavaRmiDgcClassLibrary"/>
		<rdfs:subClassOf rdf:resource="&j2se-5_0;JavaRmiRegistryClassLibrary"/>
		<rdfs:subClassOf rdf:resource="&j2se-5_0;JavaSqlClassLibrary"/>
		<rdfs:subClassOf rdf:resource="&j2se-5_0;OrgW3cDomClassLibrary"/>
		<rdfs:subClassOf rdf:resource="&j2se-5_0;OrgW3cDomLsClassLibrary"/>
		<rdfs:subClassOf rdf:resource="&j2se-5_0;OrgW3cDomBootstrapClassLibrary"/>
		<rdfs:subClassOf rdf:resource="&j2se-5_0;OrgW3cDomCssClassLibrary"/>
		<rdfs:subClassOf rdf:resource="&j2se-5_0;OrgW3cDomStylesheetsClassLibrary"/>
		<rdfs:subClassOf rdf:resource="&j2se-5_0;OrgW3cDomViewsClassLibrary"/>
		<rdfs:subClassOf rdf:resource="&j2se-5_0;OrgW3cDomEventsClassLibrary"/>
		<rdfs:subClassOf rdf:resource="&j2se-5_0;OrgW3cDomHtmlClassLibrary"/>
		<rdfs:subClassOf rdf:resource="&j2se-5_0;OrgW3cDomTraversalClassLibrary"/>
		<rdfs:subClassOf rdf:resource="&j2se-5_0;OrgW3cDomRangesClassLibrary"/>
		<rdfs:subClassOf rdf:resource="&j2se-5_0;OrgOmgCORBA_2_3ClassLibrary"/>
		<rdfs:subClassOf rdf:resource="&j2se-5_0;OrgOmgCORBA_2_3PortableClassLibrary"/>
		<rdfs:subClassOf rdf:resource="&j2se-5_0;OrgOmgCORBAClassLibrary"/>
		<rdfs:subClassOf rdf:resource="&j2se-5_0;OrgOmgCORBAPortableClassLibrary"/>
		<rdfs:subClassOf rdf:resource="&j2se-5_0;OrgOmgCORBADynAnyPackageClassLibrary"/>
		<rdfs:subClassOf rdf:resource="&j2se-5_0;OrgOmgCORBAORBPackageClassLibrary"/>
		<rdfs:subClassOf rdf:resource="&j2se-5_0;OrgOmgCORBATypeCodePackageClassLibrary"/>
		<rdfs:subClassOf rdf:resource="&j2se-5_0;OrgOmgSendingContextClassLibrary"/>
		<rdfs:subClassOf rdf:resource="&j2se-5_0;OrgOmgCosNamingClassLibrary"/>
		<rdfs:subClassOf rdf:resource="&j2se-5_0;OrgOmgCosNamingNamingContextExtPackageClassLibrary"/>
		<rdfs:subClassOf rdf:resource="&j2se-5_0;OrgOmgCosNamingNamingContextPackageClassLibrary"/>
		<rdfs:subClassOf rdf:resource="&j2se-5_0;OrgOmgPortableServerClassLibrary"/>
		<rdfs:subClassOf rdf:resource="&j2se-5_0;OrgOmgPortableServerCurrentPackageClassLibrary"/>
		<rdfs:subClassOf rdf:resource="&j2se-5_0;OrgOmgPortableServerPOAManagerPackageClassLibrary"/>
		<rdfs:subClassOf rdf:resource="&j2se-5_0;OrgOmgPortableServerPOAPackageClassLibrary"/>
		<rdfs:subClassOf rdf:resource="&j2se-5_0;OrgOmgPortableServerPortableClassLibrary"/>
		<rdfs:subClassOf rdf:resource="&j2se-5_0;OrgOmgPortableServerServantLocatorPackageClassLibrary"/>
		<rdfs:subClassOf rdf:resource="&j2se-5_0;OrgOmgDynamicClassLibrary"/>
		<rdfs:subClassOf rdf:resource="&j2se-5_0;OrgOmgDynamicAnyClassLibrary"/>
		<rdfs:subClassOf rdf:resource="&j2se-5_0;OrgOmgDynamicAnyDynAnyFactoryPackageClassLibrary"/>
		<rdfs:subClassOf rdf:resource="&j2se-5_0;OrgOmgDynamicAnyDynAnyPackageClassLibrary"/>
		<rdfs:subClassOf rdf:resource="&j2se-5_0;OrgOmgIOPClassLibrary"/>
		<rdfs:subClassOf rdf:resource="&j2se-5_0;OrgOmgIOPCodecFactoryPackageClassLibrary"/>
		<rdfs:subClassOf rdf:resource="&j2se-5_0;OrgOmgIOPCodecPackageClassLibrary"/>
		<rdfs:subClassOf rdf:resource="&j2se-5_0;OrgOmgMessagingClassLibrary"/>
		<rdfs:subClassOf rdf:resource="&j2se-5_0;OrgOmgPortableInterceptorClassLibrary"/>
		<rdfs:subClassOf rdf:resource="&j2se-5_0;OrgOmgPortableInterceptorORBInitInfoPackageClassLibrary"/>
		<rdfs:subClassOf rdf:resource="&j2se-5_0;OrgOmgStubJavaRmiClassLibrary"/>
		<rdfs:subClassOf rdf:resource="&j2se-5_0;OrgOmgStubJavaxManagementRemoteRmiClassLibrary"/>
		<rdfs:subClassOf rdf:resource="&j2se-5_0;OrgXmlSaxClassLibrary"/>
		<rdfs:subClassOf rdf:resource="&j2se-5_0;OrgXmlSaxExtClassLibrary"/>
		<rdfs:subClassOf rdf:resource="&j2se-5_0;OrgXmlSaxHelpersClassLibrary"/>
		<rdfs:subClassOf rdf:resource="&j2se-5_0;OrgIetfJgssClassLibrary"/>
		<rdfs:comment xml:lang="en">Java class library implementing the J2SE 5.0 API</rdfs:comment>
		<rdfs:comment xml:lang="OWLManchester">platform:implementsInterface some J2SE5_0API</rdfs:comment>
	</owl:Class>
	<owl:Class rdf:about="&j2se-5_0;J2SE5_0BytecodeFormat">
		<rdfs:subClassOf rdf:resource="&j2se-1_4;J2SE1_4BytecodeFormat"/>
		<rdfs:comment xml:lang="en">J2SE 5.0 bytecode format</rdfs:comment>
		<rdfs:comment xml:lang="OWLManchester">java:majorVersionNumber some xsd:integer[>="49"^^xsd:integer] and java:preverified value false</rdfs:comment>
	</owl:Class>
	<j2se-5_0:J2SE5_0BytecodeFormat rdf:about="&j2se-5_0;theJ2SE5_0BytecodeFormat">
		<java:preverified rdf:datatype="http://www.w3.org/2001/XMLSchema#boolean">false</java:preverified>
		<java:minorVersionNumber rdf:datatype="http://www.w3.org/2001/XMLSchema#integer">3</java:minorVersionNumber>
		<java:majorVersionNumber rdf:datatype="http://www.w3.org/2001/XMLSchema#integer">49</java:majorVersionNumber>
	</j2se-5_0:J2SE5_0BytecodeFormat>
	<j2se-5_0:J2SE5_0API rdf:about="&j2se-5_0;theJ2SE5_0API">
		<platform:comprisesInterfacePart rdf:resource="&j2se-5_0;theOrgIetfJgssPart"/>
		<platform:comprisesInterfacePart rdf:resource="&j2se-5_0;theOrgXmlSaxHelpersPart"/>
		<platform:comprisesInterfacePart rdf:resource="&j2se-5_0;theOrgXmlSaxExtPart"/>
		<platform:comprisesInterfacePart rdf:resource="&j2se-5_0;theOrgXmlSaxPart"/>
		<platform:comprisesInterfacePart rdf:resource="&j2se-5_0;theOrgOmgStubJavaxManagementRemoteRmiPart"/>
		<platform:comprisesInterfacePart rdf:resource="&j2se-5_0;theOrgOmgStubJavaRmiPart"/>
		<platform:comprisesInterfacePart rdf:resource="&j2se-5_0;theOrgOmgPortableInterceptorORBInitInfoPackagePart"/>
		<platform:comprisesInterfacePart rdf:resource="&j2se-5_0;theOrgOmgPortableInterceptorPart"/>
		<platform:comprisesInterfacePart rdf:resource="&j2se-5_0;theOrgOmgMessagingPart"/>
		<platform:comprisesInterfacePart rdf:resource="&j2se-5_0;theOrgOmgIOPCodecPackagePart"/>
		<platform:comprisesInterfacePart rdf:resource="&j2se-5_0;theOrgOmgIOPCodecFactoryPackagePart"/>
		<platform:comprisesInterfacePart rdf:resource="&j2se-5_0;theOrgOmgIOPPart"/>
		<platform:comprisesInterfacePart rdf:resource="&j2se-5_0;theOrgOmgDynamicAnyDynAnyPackagePart"/>
		<platform:comprisesInterfacePart rdf:resource="&j2se-5_0;theOrgOmgDynamicAnyDynAnyFactoryPackagePart"/>
		<platform:comprisesInterfacePart rdf:resource="&j2se-5_0;theOrgOmgDynamicAnyPart"/>
		<platform:comprisesInterfacePart rdf:resource="&j2se-5_0;theOrgOmgDynamicPart"/>
		<platform:comprisesInterfacePart rdf:resource="&j2se-5_0;theOrgOmgPortableServerServantLocatorPackagePart"/>
		<platform:comprisesInterfacePart rdf:resource="&j2se-5_0;theOrgOmgPortableServerPortablePart"/>
		<platform:comprisesInterfacePart rdf:resource="&j2se-5_0;theOrgOmgPortableServerPOAPackagePart"/>
		<platform:comprisesInterfacePart rdf:resource="&j2se-5_0;theOrgOmgPortableServerPOAManagerPackagePart"/>
		<platform:comprisesInterfacePart rdf:resource="&j2se-5_0;theOrgOmgPortableServerCurrentPackagePart"/>
		<platform:comprisesInterfacePart rdf:resource="&j2se-5_0;theOrgOmgPortableServerPart"/>
		<platform:comprisesInterfacePart rdf:resource="&j2se-5_0;theOrgOmgCosNamingNamingContextPackagePart"/>
		<platform:comprisesInterfacePart rdf:resource="&j2se-5_0;theOrgOmgCosNamingNamingContextExtPackagePart"/>
		<platform:comprisesInterfacePart rdf:resource="&j2se-5_0;theOrgOmgCosNamingPart"/>
		<platform:comprisesInterfacePart rdf:resource="&j2se-5_0;theOrgOmgSendingContextPart"/>
		<platform:comprisesInterfacePart rdf:resource="&j2se-5_0;theOrgOmgCORBATypeCodePackagePart"/>
		<platform:comprisesInterfacePart rdf:resource="&j2se-5_0;theOrgOmgCORBAORBPackagePart"/>
		<platform:comprisesInterfacePart rdf:resource="&j2se-5_0;theOrgOmgCORBADynAnyPackagePart"/>
		<platform:comprisesInterfacePart rdf:resource="&j2se-5_0;theOrgOmgCORBAPortablePart"/>
		<platform:comprisesInterfacePart rdf:resource="&j2se-5_0;theOrgOmgCORBAPart"/>
		<platform:comprisesInterfacePart rdf:resource="&j2se-5_0;theOrgOmgCORBA_2_3PortablePart"/>
		<platform:comprisesInterfacePart rdf:resource="&j2se-5_0;theOrgOmgCORBA_2_3Part"/>
		<platform:comprisesInterfacePart rdf:resource="&j2se-5_0;theOrgW3cDomRangesPart"/>
		<platform:comprisesInterfacePart rdf:resource="&j2se-5_0;theOrgW3cDomTraversalPart"/>
		<platform:comprisesInterfacePart rdf:resource="&j2se-5_0;theOrgW3cDomHtmlPart"/>
		<platform:comprisesInterfacePart rdf:resource="&j2se-5_0;theOrgW3cDomEventsPart"/>
		<platform:comprisesInterfacePart rdf:resource="&j2se-5_0;theOrgW3cDomViewsPart"/>
		<platform:comprisesInterfacePart rdf:resource="&j2se-5_0;theOrgW3cDomStylesheetsPart"/>
		<platform:comprisesInterfacePart rdf:resource="&j2se-5_0;theOrgW3cDomCssPart"/>
		<platform:comprisesInterfacePart rdf:resource="&j2se-5_0;theOrgW3cDomBootstrapPart"/>
		<platform:comprisesInterfacePart rdf:resource="&j2se-5_0;theOrgW3cDomLsPart"/>
		<platform:comprisesInterfacePart rdf:resource="&j2se-5_0;theOrgW3cDomPart"/>
		<platform:comprisesInterfacePart rdf:resource="&j2se-5_0;theJavaSqlPart"/>
		<platform:comprisesInterfacePart rdf:resource="&j2se-5_0;theJavaRmiRegistryPart"/>
		<platform:comprisesInterfacePart rdf:resource="&j2se-5_0;theJavaRmiDgcPart"/>
		<platform:comprisesInterfacePart rdf:resource="&j2se-5_0;theJavaRmiServerPart"/>
		<platform:comprisesInterfacePart rdf:resource="&j2se-5_0;theJavaRmiActivationPart"/>
		<platform:comprisesInterfacePart rdf:resource="&j2se-5_0;theJavaRmiPart"/>
		<platform:comprisesInterfacePart rdf:resource="&j2se-5_0;theJavaBeansBeancontextPart"/>
		<platform:comprisesInterfacePart rdf:resource="&j2se-5_0;theJavaBeansPart"/>
		<platform:comprisesInterfacePart rdf:resource="&j2se-5_0;theJavaTextPart"/>
		<platform:comprisesInterfacePart rdf:resource="&j2se-5_0;theJavaAwtPrintPart"/>
		<platform:comprisesInterfacePart rdf:resource="&j2se-5_0;theJavaAwtFontPart"/>
		<platform:comprisesInterfacePart rdf:resource="&j2se-5_0;theJavaAwtDndPart"/>
		<platform:comprisesInterfacePart rdf:resource="&j2se-5_0;theJavaAwtDatatransferPart"/>
		<platform:comprisesInterfacePart rdf:resource="&j2se-5_0;theJavaAwtColorPart"/>
		<platform:comprisesInterfacePart rdf:resource="&j2se-5_0;theJavaAwtImSpiPart"/>
		<platform:comprisesInterfacePart rdf:resource="&j2se-5_0;theJavaAwtImPart"/>
		<platform:comprisesInterfacePart rdf:resource="&j2se-5_0;theJavaAwtGeomPart"/>
		<platform:comprisesInterfacePart rdf:resource="&j2se-5_0;theJavaAwtImageRenderablePart"/>
		<platform:comprisesInterfacePart rdf:resource="&j2se-5_0;theJavaAwtImagePart"/>
		<platform:comprisesInterfacePart rdf:resource="&j2se-5_0;theJavaAwtEventPart"/>
		<platform:comprisesInterfacePart rdf:resource="&j2se-5_0;theJavaAwtPart"/>
		<platform:comprisesInterfacePart rdf:resource="&j2se-5_0;theJavaAppletPart"/>
		<platform:comprisesInterfacePart rdf:resource="&j2se-5_0;theJavaUtilPrefsPart"/>
		<platform:comprisesInterfacePart rdf:resource="&j2se-5_0;theJavaUtilLoggingPart"/>
		<platform:comprisesInterfacePart rdf:resource="&j2se-5_0;theJavaUtilZipPart"/>
		<platform:comprisesInterfacePart rdf:resource="&j2se-5_0;theJavaUtilJarPart"/>
		<platform:comprisesInterfacePart rdf:resource="&j2se-5_0;theJavaUtilConcurrentLocksPart"/>
		<platform:comprisesInterfacePart rdf:resource="&j2se-5_0;theJavaUtilConcurrentAtomicPart"/>
		<platform:comprisesInterfacePart rdf:resource="&j2se-5_0;theJavaUtilConcurrentPart"/>
		<platform:comprisesInterfacePart rdf:resource="&j2se-5_0;theJavaUtilRegexPart"/>
		<platform:comprisesInterfacePart rdf:resource="&j2se-5_0;theJavaUtilPart"/>
		<platform:comprisesInterfacePart rdf:resource="&j2se-5_0;theJavaNetPart"/>
		<platform:comprisesInterfacePart rdf:resource="&j2se-5_0;theJavaIoPart"/>
		<platform:comprisesInterfacePart rdf:resource="&j2se-5_0;theJavaNioCharsetSpiPart"/>
		<platform:comprisesInterfacePart rdf:resource="&j2se-5_0;theJavaNioCharsetPart"/>
		<platform:comprisesInterfacePart rdf:resource="&j2se-5_0;theJavaNioChannelsSpiPart"/>
		<platform:comprisesInterfacePart rdf:resource="&j2se-5_0;theJavaNioChannelsPart"/>
		<platform:comprisesInterfacePart rdf:resource="&j2se-5_0;theJavaNioPart"/>
		<platform:comprisesInterfacePart rdf:resource="&j2se-5_0;theJavaMathPart"/>
		<platform:comprisesInterfacePart rdf:resource="&j2se-5_0;theJavaSecurityInterfacesPart"/>
		<platform:comprisesInterfacePart rdf:resource="&j2se-5_0;theJavaSecurityAclPart"/>
		<platform:comprisesInterfacePart rdf:resource="&j2se-5_0;theJavaSecurityCertPart"/>
		<platform:comprisesInterfacePart rdf:resource="&j2se-5_0;theJavaSecuritySpecPart"/>
		<platform:comprisesInterfacePart rdf:resource="&j2se-5_0;theJavaSecurityPart"/>
		<platform:comprisesInterfacePart rdf:resource="&j2se-5_0;theJavaLangRefPart"/>
		<platform:comprisesInterfacePart rdf:resource="&j2se-5_0;theJavaLangManagementPart"/>
		<platform:comprisesInterfacePart rdf:resource="&j2se-5_0;theJavaLangInstrumentPart"/>
		<platform:comprisesInterfacePart rdf:resource="&j2se-5_0;theJavaLangAnnotationPart"/>
		<platform:comprisesInterfacePart rdf:resource="&j2se-5_0;theJavaLangReflectPart"/>
		<platform:comprisesInterfacePart rdf:resource="&j2se-5_0;theJavaLangPart"/>
		<platform:comprisesInterfacePart rdf:resource="&j2se-5_0;theJavaxXmlParsersPart"/>
		<platform:comprisesInterfacePart rdf:resource="&j2se-5_0;theJavaxXmlXpathPart"/>
		<platform:comprisesInterfacePart rdf:resource="&j2se-5_0;theJavaxXmlValidationPart"/>
		<platform:comprisesInterfacePart rdf:resource="&j2se-5_0;theJavaxXmlTransformStreamPart"/>
		<platform:comprisesInterfacePart rdf:resource="&j2se-5_0;theJavaxXmlTransformSaxPart"/>
		<platform:comprisesInterfacePart rdf:resource="&j2se-5_0;theJavaxXmlTransformDomPart"/>
		<platform:comprisesInterfacePart rdf:resource="&j2se-5_0;theJavaxXmlTransformPart"/>
		<platform:comprisesInterfacePart rdf:resource="&j2se-5_0;theJavaxXmlNamespacePart"/>
		<platform:comprisesInterfacePart rdf:resource="&j2se-5_0;theJavaxXmlDatatypePart"/>
		<platform:comprisesInterfacePart rdf:resource="&j2se-5_0;theJavaxXmlPart"/>
		<platform:comprisesInterfacePart rdf:resource="&j2se-5_0;theJavaxTransactionXaPart"/>
		<platform:comprisesInterfacePart rdf:resource="&j2se-5_0;theJavaxTransactionPart"/>
		<platform:comprisesInterfacePart rdf:resource="&j2se-5_0;theJavaxSqlRowsetSerialPart"/>
		<platform:comprisesInterfacePart rdf:resource="&j2se-5_0;theJavaxSqlRowsetSpiPart"/>
		<platform:comprisesInterfacePart rdf:resource="&j2se-5_0;theJavaxSqlRowsetPart"/>
		<platform:comprisesInterfacePart rdf:resource="&j2se-5_0;theJavaxSqlPart"/>
		<platform:comprisesInterfacePart rdf:resource="&j2se-5_0;theJavaxSoundSampledSpiPart"/>
		<platform:comprisesInterfacePart rdf:resource="&j2se-5_0;theJavaxSoundSampledPart"/>
		<platform:comprisesInterfacePart rdf:resource="&j2se-5_0;theJavaxSoundMidiSpiPart"/>
		<platform:comprisesInterfacePart rdf:resource="&j2se-5_0;theJavaxSoundMidiPart"/>
		<platform:comprisesInterfacePart rdf:resource="&j2se-5_0;theJavaxRmiSslPart"/>
		<platform:comprisesInterfacePart rdf:resource="&j2se-5_0;theJavaxRmiCORBAPart"/>
		<platform:comprisesInterfacePart rdf:resource="&j2se-5_0;theJavaxRmiPart"/>
		<platform:comprisesInterfacePart rdf:resource="&j2se-5_0;theJavaxPrintEventPart"/>
		<platform:comprisesInterfacePart rdf:resource="&j2se-5_0;theJavaxPrintAttributeStandardPart"/>
		<platform:comprisesInterfacePart rdf:resource="&j2se-5_0;theJavaxPrintAttributePart"/>
		<platform:comprisesInterfacePart rdf:resource="&j2se-5_0;theJavaxPrintPart"/>
		<platform:comprisesInterfacePart rdf:resource="&j2se-5_0;theJavaxNamingSpiPart"/>
		<platform:comprisesInterfacePart rdf:resource="&j2se-5_0;theJavaxNamingLdapPart"/>
		<platform:comprisesInterfacePart rdf:resource="&j2se-5_0;theJavaxNamingEventPart"/>
		<platform:comprisesInterfacePart rdf:resource="&j2se-5_0;theJavaxNamingDirectoryPart"/>
		<platform:comprisesInterfacePart rdf:resource="&j2se-5_0;theJavaxNamingPart"/>
		<platform:comprisesInterfacePart rdf:resource="&j2se-5_0;theJavaxImageioSpiPart"/>
		<platform:comprisesInterfacePart rdf:resource="&j2se-5_0;theJavaxImageioStreamPart"/>
		<platform:comprisesInterfacePart rdf:resource="&j2se-5_0;theJavaxImageioPluginsJpegPart"/>
		<platform:comprisesInterfacePart rdf:resource="&j2se-5_0;theJavaxImageioPluginsBmpPart"/>
		<platform:comprisesInterfacePart rdf:resource="&j2se-5_0;theJavaxImageioEventPart"/>
		<platform:comprisesInterfacePart rdf:resource="&j2se-5_0;theJavaxImageioMetadataPart"/>
		<platform:comprisesInterfacePart rdf:resource="&j2se-5_0;theJavaxImageioPart"/>
		<platform:comprisesInterfacePart rdf:resource="&j2se-5_0;theJavaxActivityPart"/>
		<platform:comprisesInterfacePart rdf:resource="&j2se-5_0;theJavaxManagementTimerPart"/>
		<platform:comprisesInterfacePart rdf:resource="&j2se-5_0;theJavaxManagementRemoteRmiPart"/>
		<platform:comprisesInterfacePart rdf:resource="&j2se-5_0;theJavaxManagementRemotePart"/>
		<platform:comprisesInterfacePart rdf:resource="&j2se-5_0;theJavaxManagementRelationPart"/>
		<platform:comprisesInterfacePart rdf:resource="&j2se-5_0;theJavaxManagementMonitorPart"/>
		<platform:comprisesInterfacePart rdf:resource="&j2se-5_0;theJavaxManagementModelmbeanPart"/>
		<platform:comprisesInterfacePart rdf:resource="&j2se-5_0;theJavaxManagementLoadingPart"/>
		<platform:comprisesInterfacePart rdf:resource="&j2se-5_0;theJavaxManagementOpenmbeanPart"/>
		<platform:comprisesInterfacePart rdf:resource="&j2se-5_0;theJavaxManagementPart"/>
		<platform:comprisesInterfacePart rdf:resource="&j2se-5_0;theJavaxSwingUndoPart"/>
		<platform:comprisesInterfacePart rdf:resource="&j2se-5_0;theJavaxSwingTablePart"/>
		<platform:comprisesInterfacePart rdf:resource="&j2se-5_0;theJavaxSwingFilechooserPart"/>
		<platform:comprisesInterfacePart rdf:resource="&j2se-5_0;theJavaxSwingBorderPart"/>
		<platform:comprisesInterfacePart rdf:resource="&j2se-5_0;theJavaxSwingTreePart"/>
		<platform:comprisesInterfacePart rdf:resource="&j2se-5_0;theJavaxSwingPlafSynthPart"/>
		<platform:comprisesInterfacePart rdf:resource="&j2se-5_0;theJavaxSwingPlafMultiPart"/>
		<platform:comprisesInterfacePart rdf:resource="&j2se-5_0;theJavaxSwingPlafMetalPart"/>
		<platform:comprisesInterfacePart rdf:resource="&j2se-5_0;theJavaxSwingPlafBasicPart"/>
		<platform:comprisesInterfacePart rdf:resource="&j2se-5_0;theJavaxSwingPlafPart"/>
		<platform:comprisesInterfacePart rdf:resource="&j2se-5_0;theJavaxSwingColorchooserPart"/>
		<platform:comprisesInterfacePart rdf:resource="&j2se-5_0;theJavaxSwingEventPart"/>
		<platform:comprisesInterfacePart rdf:resource="&j2se-5_0;theJavaxSwingTextRtfPart"/>
		<platform:comprisesInterfacePart rdf:resource="&j2se-5_0;theJavaxSwingTextHtmlParserPart"/>
		<platform:comprisesInterfacePart rdf:resource="&j2se-5_0;theJavaxSwingTextHtmlPart"/>
		<platform:comprisesInterfacePart rdf:resource="&j2se-5_0;theJavaxSwingTextPart"/>
		<platform:comprisesInterfacePart rdf:resource="&j2se-5_0;theJavaxSwingPart"/>
		<platform:comprisesInterfacePart rdf:resource="&j2se-5_0;theJavaxAccessibilityPart"/>
		<platform:comprisesInterfacePart rdf:resource="&j2se-5_0;theJavaxSecuritySaslPart"/>
		<platform:comprisesInterfacePart rdf:resource="&j2se-5_0;theJavaxSecurityAuthSpiPart"/>
		<platform:comprisesInterfacePart rdf:resource="&j2se-5_0;theJavaxSecurityAuthLoginPart"/>
		<platform:comprisesInterfacePart rdf:resource="&j2se-5_0;theJavaxSecurityAuthKerberosPart"/>
		<platform:comprisesInterfacePart rdf:resource="&j2se-5_0;theJavaxSecurityAuthX500Part"/>
		<platform:comprisesInterfacePart rdf:resource="&j2se-5_0;theJavaxSecurityAuthCallbackPart"/>
		<platform:comprisesInterfacePart rdf:resource="&j2se-5_0;theJavaxSecurityAuthPart"/>
		<platform:comprisesInterfacePart rdf:resource="&j2se-5_0;theJavaxSecurityCertPart"/>
		<platform:comprisesInterfacePart rdf:resource="&j2se-5_0;theJavaxNetSslPart"/>
		<platform:comprisesInterfacePart rdf:resource="&j2se-5_0;theJavaxNetPart"/>
		<platform:comprisesInterfacePart rdf:resource="&j2se-5_0;theJavaxCryptoSpecPart"/>
		<platform:comprisesInterfacePart rdf:resource="&j2se-5_0;theJavaxCryptoInterfacesPart"/>
		<platform:comprisesInterfacePart rdf:resource="&j2se-5_0;theJavaxCryptoPart"/>
	</j2se-5_0:J2SE5_0API>
	<owl:Class rdf:about="&j2se-5_0;J2SE5_0VM">
		<owl:equivalentClass>
			<owl:Restriction>
				<owl:onProperty rdf:resource="&platform;implementsInterface"/>
				<owl:someValuesFrom rdf:resource="&j2se-5_0;J2SE5_0BytecodeFormat"/>
			</owl:Restriction>
		</owl:equivalentClass>
		<rdfs:subClassOf rdf:resource="&java;JavaVM"/>
		<rdfs:comment xml:lang="en">J2SE 5.0 virtual machine</rdfs:comment>
	</owl:Class>
	<owl:Class rdf:about="&j2se-5_0;J2SE5_0JRE">
		<owl:equivalentClass>
			<owl:Class >
				<owl:intersectionOf rdf:parseType="Collection">
					<owl:Restriction>
						<owl:onProperty rdf:resource="&platform;providesFeature"/>
						<owl:someValuesFrom rdf:resource="&j2se-5_0;J2SE5_0ClassLibrary"/>
					</owl:Restriction>
					<owl:Restriction>
						<owl:onProperty rdf:resource="&platform;providesFeature"/>
						<owl:someValuesFrom rdf:resource="&j2se-5_0;J2SE5_0VM"/>
					</owl:Restriction>
				</owl:intersectionOf>
			</owl:Class>
		</owl:equivalentClass>
		<rdfs:subClassOf rdf:resource="&java;JRE"/>
		<rdfs:comment xml:lang="en">J2SE 5.0 Java Runtime Environment</rdfs:comment>
	</owl:Class>
	<owl:Class rdf:about="&j2se-5_0;JavaxCrypto">
		<rdfs:subClassOf rdf:resource="&j2se-1_4;JavaxCrypto"/>
		<rdfs:seeAlso rdf:resource="&j2se-5_0;JavaSecurity"/>
		<rdfs:seeAlso rdf:resource="&j2se-5_0;JavaIo"/>
		<rdfs:seeAlso rdf:resource="&j2se-5_0;JavaSecuritySpec"/>
		<rdfs:seeAlso rdf:resource="&j2se-5_0;JavaNio"/>
		<rdfs:seeAlso rdf:resource="&j2se-5_0;JavaLang"/>
		<rdfs:seeAlso rdf:resource="&j2se-5_0;JavaSecurityCert"/>
		<rdfs:comment xml:lang="en">Java API part implementing the javax.crypto package for J2SE 5.0</rdfs:comment>
	</owl:Class>
	<owl:Class rdf:about="&j2se-5_0;JavaxCryptoInterfaces">
		<owl:equivalentClass rdf:resource="&j2se-1_4;JavaxCryptoInterfaces"/>
		<rdfs:subClassOf rdf:resource="&java;JavaAPIPart"/>
		<rdfs:seeAlso rdf:resource="&j2se-5_0;JavaMath"/>
		<rdfs:seeAlso rdf:resource="&j2se-5_0;JavaSecurity"/>
		<rdfs:seeAlso rdf:resource="&j2se-5_0;JavaxCryptoSpec"/>
		<rdfs:seeAlso rdf:resource="&j2se-5_0;JavaxCrypto"/>
		<rdfs:comment xml:lang="en">Java API part implementing the javax.crypto.interfaces package for J2SE 5.0</rdfs:comment>
	</owl:Class>
	<owl:Class rdf:about="&j2se-5_0;JavaxCryptoSpec">
		<rdfs:subClassOf rdf:resource="&j2se-1_4;JavaxCryptoSpec"/>
		<rdfs:seeAlso rdf:resource="&j2se-5_0;JavaSecuritySpec"/>
		<rdfs:seeAlso rdf:resource="&j2se-5_0;JavaMath"/>
		<rdfs:seeAlso rdf:resource="&j2se-5_0;JavaLang"/>
		<rdfs:seeAlso rdf:resource="&j2se-5_0;JavaxCrypto"/>
		<rdfs:comment xml:lang="en">Java API part implementing the javax.crypto.spec package for J2SE 5.0</rdfs:comment>
	</owl:Class>
	<owl:Class rdf:about="&j2se-5_0;JavaxNet">
		<owl:equivalentClass rdf:resource="&j2se-1_4;JavaxNet"/>
		<rdfs:subClassOf rdf:resource="&java;JavaAPIPart"/>
		<rdfs:seeAlso rdf:resource="&j2se-5_0;JavaLang"/>
		<rdfs:seeAlso rdf:resource="&j2se-5_0;JavaNet"/>
		<rdfs:comment xml:lang="en">Java API part implementing the javax.net package for J2SE 5.0</rdfs:comment>
	</owl:Class>
	<owl:Class rdf:about="&j2se-5_0;JavaxNetSsl">
		<rdfs:subClassOf rdf:resource="&j2se-1_4;JavaxNetSsl"/>
		<rdfs:seeAlso rdf:resource="&j2se-5_0;JavaNet"/>
		<rdfs:seeAlso rdf:resource="&j2se-5_0;JavaIo"/>
		<rdfs:seeAlso rdf:resource="&j2se-5_0;JavaSecurity"/>
		<rdfs:seeAlso rdf:resource="&j2se-5_0;JavaUtil"/>
		<rdfs:seeAlso rdf:resource="&j2se-5_0;JavaxNet"/>
		<rdfs:seeAlso rdf:resource="&j2se-5_0;JavaNio"/>
		<rdfs:seeAlso rdf:resource="&j2se-5_0;JavaLang"/>
		<rdfs:seeAlso rdf:resource="&j2se-5_0;JavaSecurityCert"/>
		<rdfs:comment xml:lang="en">Java API part implementing the javax.net.ssl package for J2SE 5.0</rdfs:comment>
	</owl:Class>
	<owl:Class rdf:about="&j2se-5_0;JavaxSecurityCert">
		<owl:equivalentClass rdf:resource="&j2se-1_4;JavaxSecurityCert"/>
		<rdfs:subClassOf rdf:resource="&java;JavaAPIPart"/>
		<rdfs:seeAlso rdf:resource="&j2se-5_0;JavaMath"/>
		<rdfs:seeAlso rdf:resource="&j2se-5_0;JavaSecurity"/>
		<rdfs:seeAlso rdf:resource="&j2se-5_0;JavaLang"/>
		<rdfs:seeAlso rdf:resource="&j2se-5_0;JavaUtil"/>
		<rdfs:seeAlso rdf:resource="&j2se-5_0;JavaIo"/>
		<rdfs:comment xml:lang="en">Java API part implementing the javax.security.cert package for J2SE 5.0</rdfs:comment>
	</owl:Class>
	<owl:Class rdf:about="&j2se-5_0;JavaxSecurityAuth">
		<owl:equivalentClass rdf:resource="&j2se-1_4;JavaxSecurityAuth"/>
		<rdfs:subClassOf rdf:resource="&java;JavaAPIPart"/>
		<rdfs:seeAlso rdf:resource="&j2se-5_0;JavaSecurity"/>
		<rdfs:seeAlso rdf:resource="&j2se-5_0;JavaUtil"/>
		<rdfs:seeAlso rdf:resource="&j2se-5_0;JavaIo"/>
		<rdfs:seeAlso rdf:resource="&j2se-5_0;JavaLang"/>
		<rdfs:comment xml:lang="en">Java API part implementing the javax.security.auth package for J2SE 5.0</rdfs:comment>
	</owl:Class>
	<owl:Class rdf:about="&j2se-5_0;JavaxSecurityAuthCallback">
		<owl:equivalentClass rdf:resource="&j2se-1_4;JavaxSecurityAuthCallback"/>
		<rdfs:subClassOf rdf:resource="&java;JavaAPIPart"/>
		<rdfs:seeAlso rdf:resource="&j2se-5_0;JavaLang"/>
		<rdfs:seeAlso rdf:resource="&j2se-5_0;JavaUtil"/>
		<rdfs:seeAlso rdf:resource="&j2se-5_0;JavaIo"/>
		<rdfs:comment xml:lang="en">Java API part implementing the javax.security.auth.callback package for J2SE 5.0</rdfs:comment>
	</owl:Class>
	<owl:Class rdf:about="&j2se-5_0;JavaxSecurityAuthX500">
		<owl:equivalentClass rdf:resource="&j2se-1_4;JavaxSecurityAuthX500"/>
		<rdfs:subClassOf rdf:resource="&java;JavaAPIPart"/>
		<rdfs:seeAlso rdf:resource="&j2se-5_0;JavaSecurity"/>
		<rdfs:seeAlso rdf:resource="&j2se-5_0;JavaLang"/>
		<rdfs:seeAlso rdf:resource="&j2se-5_0;JavaSecurityCert"/>
		<rdfs:seeAlso rdf:resource="&j2se-5_0;JavaIo"/>
		<rdfs:seeAlso rdf:resource="&j2se-5_0;JavaxSecurityAuth"/>
		<rdfs:comment xml:lang="en">Java API part implementing the javax.security.auth.x500 package for J2SE 5.0</rdfs:comment>
	</owl:Class>
	<owl:Class rdf:about="&j2se-5_0;JavaxSecurityAuthKerberos">
		<owl:equivalentClass rdf:resource="&j2se-1_4;JavaxSecurityAuthKerberos"/>
		<rdfs:subClassOf rdf:resource="&java;JavaAPIPart"/>
		<rdfs:seeAlso rdf:resource="&j2se-5_0;JavaSecurity"/>
		<rdfs:seeAlso rdf:resource="&j2se-5_0;JavaLang"/>
		<rdfs:seeAlso rdf:resource="&j2se-5_0;JavaUtil"/>
		<rdfs:seeAlso rdf:resource="&j2se-5_0;JavaxCrypto"/>
		<rdfs:seeAlso rdf:resource="&j2se-5_0;JavaIo"/>
		<rdfs:seeAlso rdf:resource="&j2se-5_0;JavaxSecurityAuth"/>
		<rdfs:comment xml:lang="en">Java API part implementing the javax.security.auth.kerberos package for J2SE 5.0</rdfs:comment>
	</owl:Class>
	<owl:Class rdf:about="&j2se-5_0;JavaxSecurityAuthLogin">
		<rdfs:subClassOf rdf:resource="&j2se-1_4;JavaxSecurityAuthLogin"/>
		<rdfs:seeAlso rdf:resource="&j2se-5_0;JavaSecurity"/>
		<rdfs:seeAlso rdf:resource="&j2se-5_0;JavaxSecurityAuthCallback"/>
		<rdfs:seeAlso rdf:resource="&j2se-5_0;JavaLang"/>
		<rdfs:seeAlso rdf:resource="&j2se-5_0;JavaUtil"/>
		<rdfs:seeAlso rdf:resource="&j2se-5_0;JavaxSecurityAuth"/>
		<rdfs:comment xml:lang="en">Java API part implementing the javax.security.auth.login package for J2SE 5.0</rdfs:comment>
	</owl:Class>
	<owl:Class rdf:about="&j2se-5_0;JavaxSecurityAuthSpi">
		<owl:equivalentClass rdf:resource="&j2se-1_4;JavaxSecurityAuthSpi"/>
		<rdfs:subClassOf rdf:resource="&java;JavaAPIPart"/>
		<rdfs:seeAlso rdf:resource="&j2se-5_0;JavaxSecurityAuthCallback"/>
		<rdfs:seeAlso rdf:resource="&j2se-5_0;JavaUtil"/>
		<rdfs:seeAlso rdf:resource="&j2se-5_0;JavaxSecurityAuth"/>
		<rdfs:comment xml:lang="en">Java API part implementing the javax.security.auth.spi package for J2SE 5.0</rdfs:comment>
	</owl:Class>
	<owl:Class rdf:about="&j2se-5_0;JavaxSecuritySasl">
		<rdfs:subClassOf rdf:resource="&java;JavaAPIPart"/>
		<rdfs:seeAlso rdf:resource="&j2se-5_0;JavaLang"/>
		<rdfs:seeAlso rdf:resource="&j2se-5_0;JavaxSecurityAuthCallback"/>
		<rdfs:seeAlso rdf:resource="&j2se-5_0;JavaUtil"/>
		<rdfs:seeAlso rdf:resource="&j2se-5_0;JavaIo"/>
		<rdfs:comment xml:lang="en">Java API part implementing the javax.security.sasl package for J2SE 5.0</rdfs:comment>
	</owl:Class>
	<owl:Class rdf:about="&j2se-5_0;JavaxAccessibility">
		<rdfs:subClassOf rdf:resource="&j2se-1_4;JavaxAccessibility"/>
		<rdfs:seeAlso rdf:resource="&j2se-5_0;JavaAwt"/>
		<rdfs:seeAlso rdf:resource="&j2se-5_0;JavaAwtDatatransfer"/>
		<rdfs:seeAlso rdf:resource="&j2se-5_0;JavaUtil"/>
		<rdfs:seeAlso rdf:resource="&j2se-5_0;JavaIo"/>
		<rdfs:seeAlso rdf:resource="&j2se-5_0;JavaAwtEvent"/>
		<rdfs:seeAlso rdf:resource="&j2se-5_0;JavaxSwingText"/>
		<rdfs:seeAlso rdf:resource="&j2se-5_0;JavaLang"/>
		<rdfs:seeAlso rdf:resource="&j2se-5_0;JavaBeans"/>
		<rdfs:comment xml:lang="en">Java API part implementing the javax.accessibility package for J2SE 5.0</rdfs:comment>
	</owl:Class>
	<owl:Class rdf:about="&j2se-5_0;JavaxSwing">
		<rdfs:subClassOf rdf:resource="&j2se-1_4;JavaxSwing"/>
		<rdfs:seeAlso rdf:resource="&j2se-5_0;JavaxSwingPlaf"/>
		<rdfs:seeAlso rdf:resource="&j2se-5_0;JavaxSwingTable"/>
		<rdfs:seeAlso rdf:resource="&j2se-5_0;JavaxSwingColorchooser"/>
		<rdfs:seeAlso rdf:resource="&j2se-5_0;JavaAwtEvent"/>
		<rdfs:seeAlso rdf:resource="&j2se-5_0;JavaxSwingBorder"/>
		<rdfs:seeAlso rdf:resource="&j2se-5_0;JavaBeans"/>
		<rdfs:seeAlso rdf:resource="&j2se-5_0;JavaxSwingTree"/>
		<rdfs:seeAlso rdf:resource="&j2se-5_0;JavaIo"/>
		<rdfs:seeAlso rdf:resource="&j2se-5_0;JavaAwtDatatransfer"/>
		<rdfs:seeAlso rdf:resource="&j2se-5_0;JavaNet"/>
		<rdfs:seeAlso rdf:resource="&j2se-5_0;JavaxSwingText"/>
		<rdfs:seeAlso rdf:resource="&j2se-5_0;JavaAwtPrint"/>
		<rdfs:seeAlso rdf:resource="&j2se-5_0;JavaUtil"/>
		<rdfs:seeAlso rdf:resource="&j2se-5_0;JavaApplet"/>
		<rdfs:seeAlso rdf:resource="&j2se-5_0;JavaxPrintAttribute"/>
		<rdfs:seeAlso rdf:resource="&j2se-5_0;JavaLang"/>
		<rdfs:seeAlso rdf:resource="&j2se-5_0;JavaxSwingFilechooser"/>
		<rdfs:seeAlso rdf:resource="&j2se-5_0;JavaxAccessibility"/>
		<rdfs:seeAlso rdf:resource="&j2se-5_0;JavaxSwingEvent"/>
		<rdfs:seeAlso rdf:resource="&j2se-5_0;JavaAwtImage"/>
		<rdfs:seeAlso rdf:resource="&j2se-5_0;JavaAwt"/>
		<rdfs:seeAlso rdf:resource="&j2se-5_0;JavaText"/>
		<rdfs:comment xml:lang="en">Java API part implementing the javax.swing package for J2SE 5.0</rdfs:comment>
	</owl:Class>
	<owl:Class rdf:about="&j2se-5_0;JavaxSwingText">
		<rdfs:subClassOf rdf:resource="&j2se-1_4;JavaxSwingText"/>
		<rdfs:seeAlso rdf:resource="&j2se-5_0;JavaxSwingPlaf"/>
		<rdfs:seeAlso rdf:resource="&j2se-5_0;JavaxSwing"/>
		<rdfs:seeAlso rdf:resource="&j2se-5_0;JavaxSwingUndo"/>
		<rdfs:seeAlso rdf:resource="&j2se-5_0;JavaAwtEvent"/>
		<rdfs:seeAlso rdf:resource="&j2se-5_0;JavaxSwingTree"/>
		<rdfs:seeAlso rdf:resource="&j2se-5_0;JavaxAccessibility"/>
		<rdfs:seeAlso rdf:resource="&j2se-5_0;JavaIo"/>
		<rdfs:seeAlso rdf:resource="&j2se-5_0;JavaxSwingPlafBasic"/>
		<rdfs:seeAlso rdf:resource="&j2se-5_0;JavaxSwingEvent"/>
		<rdfs:seeAlso rdf:resource="&j2se-5_0;JavaAwt"/>
		<rdfs:seeAlso rdf:resource="&j2se-5_0;JavaUtil"/>
		<rdfs:seeAlso rdf:resource="&j2se-5_0;JavaText"/>
		<rdfs:seeAlso rdf:resource="&j2se-5_0;JavaLang"/>
		<rdfs:seeAlso rdf:resource="&j2se-5_0;JavaAwtIm"/>
		<rdfs:comment xml:lang="en">Java API part implementing the javax.swing.text package for J2SE 5.0</rdfs:comment>
	</owl:Class>
	<owl:Class rdf:about="&j2se-5_0;JavaxSwingTextHtml">
		<rdfs:subClassOf rdf:resource="&j2se-1_4;JavaxSwingTextHtml"/>
		<rdfs:seeAlso rdf:resource="&j2se-5_0;JavaNet"/>
		<rdfs:seeAlso rdf:resource="&j2se-5_0;JavaxSwing"/>
		<rdfs:seeAlso rdf:resource="&j2se-5_0;JavaxSwingText"/>
		<rdfs:seeAlso rdf:resource="&j2se-5_0;JavaAwtEvent"/>
		<rdfs:seeAlso rdf:resource="&j2se-5_0;JavaxAccessibility"/>
		<rdfs:seeAlso rdf:resource="&j2se-5_0;JavaIo"/>
		<rdfs:seeAlso rdf:resource="&j2se-5_0;JavaxSwingEvent"/>
		<rdfs:seeAlso rdf:resource="&j2se-5_0;JavaAwt"/>
		<rdfs:seeAlso rdf:resource="&j2se-5_0;JavaUtil"/>
		<rdfs:seeAlso rdf:resource="&j2se-5_0;JavaLang"/>
		<rdfs:comment xml:lang="en">Java API part implementing the javax.swing.text.html package for J2SE 5.0</rdfs:comment>
	</owl:Class>
	<owl:Class rdf:about="&j2se-5_0;JavaxSwingTextHtmlParser">
		<owl:equivalentClass rdf:resource="&j2se-1_4;JavaxSwingTextHtmlParser"/>
		<rdfs:subClassOf rdf:resource="&java;JavaAPIPart"/>
		<rdfs:seeAlso rdf:resource="&j2se-5_0;JavaxSwingTextHtml"/>
		<rdfs:seeAlso rdf:resource="&j2se-5_0;JavaUtil"/>
		<rdfs:seeAlso rdf:resource="&j2se-5_0;JavaIo"/>
		<rdfs:seeAlso rdf:resource="&j2se-5_0;JavaxSwingText"/>
		<rdfs:seeAlso rdf:resource="&j2se-5_0;JavaLang"/>
		<rdfs:comment xml:lang="en">Java API part implementing the javax.swing.text.html.parser package for J2SE 5.0</rdfs:comment>
	</owl:Class>
	<owl:Class rdf:about="&j2se-5_0;JavaxSwingTextRtf">
		<owl:equivalentClass rdf:resource="&j2se-1_4;JavaxSwingTextRtf"/>
		<rdfs:subClassOf rdf:resource="&java;JavaAPIPart"/>
		<rdfs:seeAlso rdf:resource="&j2se-5_0;JavaxSwingText"/>
		<rdfs:seeAlso rdf:resource="&j2se-5_0;JavaLang"/>
		<rdfs:seeAlso rdf:resource="&j2se-5_0;JavaIo"/>
		<rdfs:comment xml:lang="en">Java API part implementing the javax.swing.text.rtf package for J2SE 5.0</rdfs:comment>
	</owl:Class>
	<owl:Class rdf:about="&j2se-5_0;JavaxSwingEvent">
		<rdfs:subClassOf rdf:resource="&j2se-1_4;JavaxSwingEvent"/>
		<rdfs:seeAlso rdf:resource="&j2se-5_0;JavaxSwingTree"/>
		<rdfs:seeAlso rdf:resource="&j2se-5_0;JavaNet"/>
		<rdfs:seeAlso rdf:resource="&j2se-5_0;JavaIo"/>
		<rdfs:seeAlso rdf:resource="&j2se-5_0;JavaxSwing"/>
		<rdfs:seeAlso rdf:resource="&j2se-5_0;JavaxSwingText"/>
		<rdfs:seeAlso rdf:resource="&j2se-5_0;JavaxSwingTable"/>
		<rdfs:seeAlso rdf:resource="&j2se-5_0;JavaAwt"/>
		<rdfs:seeAlso rdf:resource="&j2se-5_0;JavaxSwingUndo"/>
		<rdfs:seeAlso rdf:resource="&j2se-5_0;JavaUtil"/>
		<rdfs:seeAlso rdf:resource="&j2se-5_0;JavaAwtEvent"/>
		<rdfs:seeAlso rdf:resource="&j2se-5_0;JavaLang"/>
		<rdfs:seeAlso rdf:resource="&j2se-5_0;JavaBeans"/>
		<rdfs:comment xml:lang="en">Java API part implementing the javax.swing.event package for J2SE 5.0</rdfs:comment>
	</owl:Class>
	<owl:Class rdf:about="&j2se-5_0;JavaxSwingColorchooser">
		<rdfs:subClassOf rdf:resource="&j2se-1_4;JavaxSwingColorchooser"/>
		<rdfs:seeAlso rdf:resource="&j2se-5_0;JavaAwt"/>
		<rdfs:seeAlso rdf:resource="&j2se-5_0;JavaIo"/>
		<rdfs:seeAlso rdf:resource="&j2se-5_0;JavaxSwing"/>
		<rdfs:seeAlso rdf:resource="&j2se-5_0;JavaxSwingEvent"/>
		<rdfs:seeAlso rdf:resource="&j2se-5_0;JavaLang"/>
		<rdfs:comment xml:lang="en">Java API part implementing the javax.swing.colorchooser package for J2SE 5.0</rdfs:comment>
	</owl:Class>
	<owl:Class rdf:about="&j2se-5_0;JavaxSwingPlaf">
		<rdfs:subClassOf rdf:resource="&j2se-1_4;JavaxSwingPlaf"/>
		<rdfs:seeAlso rdf:resource="&j2se-5_0;JavaxSwingTree"/>
		<rdfs:seeAlso rdf:resource="&j2se-5_0;JavaxSwingFilechooser"/>
		<rdfs:seeAlso rdf:resource="&j2se-5_0;JavaxAccessibility"/>
		<rdfs:seeAlso rdf:resource="&j2se-5_0;JavaxSwing"/>
		<rdfs:seeAlso rdf:resource="&j2se-5_0;JavaIo"/>
		<rdfs:seeAlso rdf:resource="&j2se-5_0;JavaxSwingBorder"/>
		<rdfs:seeAlso rdf:resource="&j2se-5_0;JavaxSwingText"/>
		<rdfs:seeAlso rdf:resource="&j2se-5_0;JavaAwt"/>
		<rdfs:seeAlso rdf:resource="&j2se-5_0;JavaAwtEvent"/>
		<rdfs:seeAlso rdf:resource="&j2se-5_0;JavaLang"/>
		<rdfs:comment xml:lang="en">Java API part implementing the javax.swing.plaf package for J2SE 5.0</rdfs:comment>
	</owl:Class>
	<owl:Class rdf:about="&j2se-5_0;JavaxSwingPlafBasic">
		<rdfs:subClassOf rdf:resource="&j2se-1_4;JavaxSwingPlafBasic"/>
		<rdfs:seeAlso rdf:resource="&j2se-5_0;JavaxSwingPlaf"/>
		<rdfs:seeAlso rdf:resource="&j2se-5_0;JavaxSwing"/>
		<rdfs:seeAlso rdf:resource="&j2se-5_0;JavaxSwingText"/>
		<rdfs:seeAlso rdf:resource="&j2se-5_0;JavaxSwingTable"/>
		<rdfs:seeAlso rdf:resource="&j2se-5_0;JavaAwtEvent"/>
		<rdfs:seeAlso rdf:resource="&j2se-5_0;JavaxSwingBorder"/>
		<rdfs:seeAlso rdf:resource="&j2se-5_0;JavaUtil"/>
		<rdfs:seeAlso rdf:resource="&j2se-5_0;JavaLang"/>
		<rdfs:seeAlso rdf:resource="&j2se-5_0;JavaxSwingFilechooser"/>
		<rdfs:seeAlso rdf:resource="&j2se-5_0;JavaBeans"/>
		<rdfs:seeAlso rdf:resource="&j2se-5_0;JavaxSwingTree"/>
		<rdfs:seeAlso rdf:resource="&j2se-5_0;JavaxAccessibility"/>
		<rdfs:seeAlso rdf:resource="&j2se-5_0;JavaIo"/>
		<rdfs:seeAlso rdf:resource="&j2se-5_0;JavaxSwingEvent"/>
		<rdfs:seeAlso rdf:resource="&j2se-5_0;JavaAwt"/>
		<rdfs:comment xml:lang="en">Java API part implementing the javax.swing.plaf.basic package for J2SE 5.0</rdfs:comment>
	</owl:Class>
	<owl:Class rdf:about="&j2se-5_0;JavaxSwingPlafMetal">
		<rdfs:subClassOf rdf:resource="&j2se-1_4;JavaxSwingPlafMetal"/>
		<rdfs:seeAlso rdf:resource="&j2se-5_0;JavaxSwingPlaf"/>
		<rdfs:seeAlso rdf:resource="&j2se-5_0;JavaxSwing"/>
		<rdfs:seeAlso rdf:resource="&j2se-5_0;JavaAwtEvent"/>
		<rdfs:seeAlso rdf:resource="&j2se-5_0;JavaBeans"/>
		<rdfs:seeAlso rdf:resource="&j2se-5_0;JavaxSwingTree"/>
		<rdfs:seeAlso rdf:resource="&j2se-5_0;JavaIo"/>
		<rdfs:seeAlso rdf:resource="&j2se-5_0;JavaxSwingBorder"/>
		<rdfs:seeAlso rdf:resource="&j2se-5_0;JavaxSwingPlafBasic"/>
		<rdfs:seeAlso rdf:resource="&j2se-5_0;JavaxSwingEvent"/>
		<rdfs:seeAlso rdf:resource="&j2se-5_0;JavaAwt"/>
		<rdfs:seeAlso rdf:resource="&j2se-5_0;JavaLang"/>
		<rdfs:comment xml:lang="en">Java API part implementing the javax.swing.plaf.metal package for J2SE 5.0</rdfs:comment>
	</owl:Class>
	<owl:Class rdf:about="&j2se-5_0;JavaxSwingPlafMulti">
		<rdfs:subClassOf rdf:resource="&j2se-1_4;JavaxSwingPlafMulti"/>
		<rdfs:seeAlso rdf:resource="&j2se-5_0;JavaxSwingFilechooser"/>
		<rdfs:seeAlso rdf:resource="&j2se-5_0;JavaxSwingPlaf"/>
		<rdfs:seeAlso rdf:resource="&j2se-5_0;JavaxSwing"/>
		<rdfs:seeAlso rdf:resource="&j2se-5_0;JavaxSwingText"/>
		<rdfs:seeAlso rdf:resource="&j2se-5_0;JavaAwtEvent"/>
		<rdfs:seeAlso rdf:resource="&j2se-5_0;JavaxSwingTree"/>
		<rdfs:seeAlso rdf:resource="&j2se-5_0;JavaxAccessibility"/>
		<rdfs:seeAlso rdf:resource="&j2se-5_0;JavaIo"/>
		<rdfs:seeAlso rdf:resource="&j2se-5_0;JavaAwt"/>
		<rdfs:seeAlso rdf:resource="&j2se-5_0;JavaUtil"/>
		<rdfs:seeAlso rdf:resource="&j2se-5_0;JavaLang"/>
		<rdfs:comment xml:lang="en">Java API part implementing the javax.swing.plaf.multi package for J2SE 5.0</rdfs:comment>
	</owl:Class>
	<owl:Class rdf:about="&j2se-5_0;JavaxSwingPlafSynth">
		<rdfs:subClassOf rdf:resource="&java;JavaAPIPart"/>
		<rdfs:seeAlso rdf:resource="&j2se-5_0;JavaAwt"/>
		<rdfs:seeAlso rdf:resource="&j2se-5_0;JavaxSwingPlaf"/>
		<rdfs:seeAlso rdf:resource="&j2se-5_0;JavaxSwing"/>
		<rdfs:seeAlso rdf:resource="&j2se-5_0;JavaIo"/>
		<rdfs:seeAlso rdf:resource="&j2se-5_0;JavaxSwingPlafBasic"/>
		<rdfs:seeAlso rdf:resource="&j2se-5_0;JavaAwtEvent"/>
		<rdfs:seeAlso rdf:resource="&j2se-5_0;JavaLang"/>
		<rdfs:comment xml:lang="en">Java API part implementing the javax.swing.plaf.synth package for J2SE 5.0</rdfs:comment>
	</owl:Class>
	<owl:Class rdf:about="&j2se-5_0;JavaxSwingTree">
		<rdfs:subClassOf rdf:resource="&j2se-1_4;JavaxSwingTree"/>
		<rdfs:seeAlso rdf:resource="&j2se-5_0;JavaIo"/>
		<rdfs:seeAlso rdf:resource="&j2se-5_0;JavaxSwing"/>
		<rdfs:seeAlso rdf:resource="&j2se-5_0;JavaxSwingBorder"/>
		<rdfs:seeAlso rdf:resource="&j2se-5_0;JavaxSwingEvent"/>
		<rdfs:seeAlso rdf:resource="&j2se-5_0;JavaAwt"/>
		<rdfs:seeAlso rdf:resource="&j2se-5_0;JavaUtil"/>
		<rdfs:seeAlso rdf:resource="&j2se-5_0;JavaAwtEvent"/>
		<rdfs:seeAlso rdf:resource="&j2se-5_0;JavaLang"/>
		<rdfs:seeAlso rdf:resource="&j2se-5_0;JavaBeans"/>
		<rdfs:comment xml:lang="en">Java API part implementing the javax.swing.tree package for J2SE 5.0</rdfs:comment>
	</owl:Class>
	<owl:Class rdf:about="&j2se-5_0;JavaxSwingBorder">
		<owl:equivalentClass rdf:resource="&j2se-1_4;JavaxSwingBorder"/>
		<rdfs:subClassOf rdf:resource="&java;JavaAPIPart"/>
		<rdfs:seeAlso rdf:resource="&j2se-5_0;JavaAwt"/>
		<rdfs:seeAlso rdf:resource="&j2se-5_0;JavaLang"/>
		<rdfs:seeAlso rdf:resource="&j2se-5_0;JavaxSwing"/>
		<rdfs:seeAlso rdf:resource="&j2se-5_0;JavaIo"/>
		<rdfs:comment xml:lang="en">Java API part implementing the javax.swing.border package for J2SE 5.0</rdfs:comment>
	</owl:Class>
	<owl:Class rdf:about="&j2se-5_0;JavaxSwingFilechooser">
		<owl:equivalentClass rdf:resource="&j2se-1_4;JavaxSwingFilechooser"/>
		<rdfs:subClassOf rdf:resource="&java;JavaAPIPart"/>
		<rdfs:seeAlso rdf:resource="&j2se-5_0;JavaLang"/>
		<rdfs:seeAlso rdf:resource="&j2se-5_0;JavaxSwing"/>
		<rdfs:seeAlso rdf:resource="&j2se-5_0;JavaIo"/>
		<rdfs:comment xml:lang="en">Java API part implementing the javax.swing.filechooser package for J2SE 5.0</rdfs:comment>
	</owl:Class>
	<owl:Class rdf:about="&j2se-5_0;JavaxSwingTable">
		<rdfs:subClassOf rdf:resource="&j2se-1_4;JavaxSwingTable"/>
		<rdfs:seeAlso rdf:resource="&j2se-5_0;JavaxSwingPlaf"/>
		<rdfs:seeAlso rdf:resource="&j2se-5_0;JavaxAccessibility"/>
		<rdfs:seeAlso rdf:resource="&j2se-5_0;JavaxSwing"/>
		<rdfs:seeAlso rdf:resource="&j2se-5_0;JavaIo"/>
		<rdfs:seeAlso rdf:resource="&j2se-5_0;JavaxSwingBorder"/>
		<rdfs:seeAlso rdf:resource="&j2se-5_0;JavaxSwingEvent"/>
		<rdfs:seeAlso rdf:resource="&j2se-5_0;JavaAwt"/>
		<rdfs:seeAlso rdf:resource="&j2se-5_0;JavaUtil"/>
		<rdfs:seeAlso rdf:resource="&j2se-5_0;JavaAwtEvent"/>
		<rdfs:seeAlso rdf:resource="&j2se-5_0;JavaLang"/>
		<rdfs:seeAlso rdf:resource="&j2se-5_0;JavaBeans"/>
		<rdfs:comment xml:lang="en">Java API part implementing the javax.swing.table package for J2SE 5.0</rdfs:comment>
	</owl:Class>
	<owl:Class rdf:about="&j2se-5_0;JavaxSwingUndo">
		<owl:equivalentClass rdf:resource="&j2se-1_4;JavaxSwingUndo"/>
		<rdfs:subClassOf rdf:resource="&java;JavaAPIPart"/>
		<rdfs:seeAlso rdf:resource="&j2se-5_0;JavaxSwingEvent"/>
		<rdfs:seeAlso rdf:resource="&j2se-5_0;JavaLang"/>
		<rdfs:seeAlso rdf:resource="&j2se-5_0;JavaUtil"/>
		<rdfs:seeAlso rdf:resource="&j2se-5_0;JavaIo"/>
		<rdfs:comment xml:lang="en">Java API part implementing the javax.swing.undo package for J2SE 5.0</rdfs:comment>
	</owl:Class>
	<owl:Class rdf:about="&j2se-5_0;JavaxManagement">
		<rdfs:subClassOf rdf:resource="&java;JavaAPIPart"/>
		<rdfs:seeAlso rdf:resource="&j2se-5_0;JavaIo"/>
		<rdfs:seeAlso rdf:resource="&j2se-5_0;JavaxManagementLoading"/>
		<rdfs:seeAlso rdf:resource="&j2se-5_0;JavaLangReflect"/>
		<rdfs:seeAlso rdf:resource="&j2se-5_0;JavaSecurity"/>
		<rdfs:seeAlso rdf:resource="&j2se-5_0;JavaUtil"/>
		<rdfs:seeAlso rdf:resource="&j2se-5_0;JavaLang"/>
		<rdfs:comment xml:lang="en">Java API part implementing the javax.management package for J2SE 5.0</rdfs:comment>
	</owl:Class>
	<owl:Class rdf:about="&j2se-5_0;JavaxManagementOpenmbean">
		<rdfs:subClassOf rdf:resource="&java;JavaAPIPart"/>
		<rdfs:seeAlso rdf:resource="&j2se-5_0;JavaUtil"/>
		<rdfs:seeAlso rdf:resource="&j2se-5_0;JavaIo"/>
		<rdfs:seeAlso rdf:resource="&j2se-5_0;JavaxManagement"/>
		<rdfs:seeAlso rdf:resource="&j2se-5_0;JavaLang"/>
		<rdfs:comment xml:lang="en">Java API part implementing the javax.management.openmbean package for J2SE 5.0</rdfs:comment>
	</owl:Class>
	<owl:Class rdf:about="&j2se-5_0;JavaxManagementLoading">
		<rdfs:subClassOf rdf:resource="&java;JavaAPIPart"/>
		<rdfs:seeAlso rdf:resource="&j2se-5_0;JavaUtil"/>
		<rdfs:seeAlso rdf:resource="&j2se-5_0;JavaNet"/>
		<rdfs:seeAlso rdf:resource="&j2se-5_0;JavaIo"/>
		<rdfs:seeAlso rdf:resource="&j2se-5_0;JavaxManagement"/>
		<rdfs:seeAlso rdf:resource="&j2se-5_0;JavaLang"/>
		<rdfs:comment xml:lang="en">Java API part implementing the javax.management.loading package for J2SE 5.0</rdfs:comment>
	</owl:Class>
	<owl:Class rdf:about="&j2se-5_0;JavaxManagementModelmbean">
		<rdfs:subClassOf rdf:resource="&java;JavaAPIPart"/>
		<rdfs:seeAlso rdf:resource="&j2se-5_0;JavaIo"/>
		<rdfs:seeAlso rdf:resource="&j2se-5_0;JavaxManagement"/>
		<rdfs:seeAlso rdf:resource="&j2se-5_0;JavaxManagementLoading"/>
		<rdfs:seeAlso rdf:resource="&j2se-5_0;JavaLangReflect"/>
		<rdfs:seeAlso rdf:resource="&j2se-5_0;JavaLang"/>
		<rdfs:comment xml:lang="en">Java API part implementing the javax.management.modelmbean package for J2SE 5.0</rdfs:comment>
	</owl:Class>
	<owl:Class rdf:about="&j2se-5_0;JavaxManagementMonitor">
		<rdfs:subClassOf rdf:resource="&java;JavaAPIPart"/>
		<rdfs:seeAlso rdf:resource="&j2se-5_0;JavaxManagement"/>
		<rdfs:seeAlso rdf:resource="&j2se-5_0;JavaLang"/>
		<rdfs:comment xml:lang="en">Java API part implementing the javax.management.monitor package for J2SE 5.0</rdfs:comment>
	</owl:Class>
	<owl:Class rdf:about="&j2se-5_0;JavaxManagementRelation">
		<rdfs:subClassOf rdf:resource="&java;JavaAPIPart"/>
		<rdfs:seeAlso rdf:resource="&j2se-5_0;JavaUtil"/>
		<rdfs:seeAlso rdf:resource="&j2se-5_0;JavaIo"/>
		<rdfs:seeAlso rdf:resource="&j2se-5_0;JavaLang"/>
		<rdfs:seeAlso rdf:resource="&j2se-5_0;JavaxManagement"/>
		<rdfs:comment xml:lang="en">Java API part implementing the javax.management.relation package for J2SE 5.0</rdfs:comment>
	</owl:Class>
	<owl:Class rdf:about="&j2se-5_0;JavaxManagementRemote">
		<rdfs:subClassOf rdf:resource="&java;JavaAPIPart"/>
		<rdfs:seeAlso rdf:resource="&j2se-5_0;JavaSecurity"/>
		<rdfs:seeAlso rdf:resource="&j2se-5_0;JavaUtil"/>
		<rdfs:seeAlso rdf:resource="&j2se-5_0;JavaIo"/>
		<rdfs:seeAlso rdf:resource="&j2se-5_0;JavaxSecurityAuth"/>
		<rdfs:seeAlso rdf:resource="&j2se-5_0;JavaLang"/>
		<rdfs:seeAlso rdf:resource="&j2se-5_0;JavaxManagement"/>
		<rdfs:comment xml:lang="en">Java API part implementing the javax.management.remote package for J2SE 5.0</rdfs:comment>
	</owl:Class>
	<owl:Class rdf:about="&j2se-5_0;JavaxManagementRemoteRmi">
		<rdfs:subClassOf rdf:resource="&java;JavaAPIPart"/>
		<rdfs:seeAlso rdf:resource="&j2se-5_0;JavaIo"/>
		<rdfs:seeAlso rdf:resource="&j2se-5_0;JavaxSecurityAuth"/>
		<rdfs:seeAlso rdf:resource="&j2se-5_0;JavaxManagement"/>
		<rdfs:seeAlso rdf:resource="&j2se-5_0;JavaxManagementRemote"/>
		<rdfs:seeAlso rdf:resource="&j2se-5_0;JavaRmi"/>
		<rdfs:seeAlso rdf:resource="&j2se-5_0;JavaUtil"/>
		<rdfs:seeAlso rdf:resource="&j2se-5_0;JavaRmiServer"/>
		<rdfs:seeAlso rdf:resource="&j2se-5_0;JavaLang"/>
		<rdfs:comment xml:lang="en">Java API part implementing the javax.management.remote.rmi package for J2SE 5.0</rdfs:comment>
	</owl:Class>
	<owl:Class rdf:about="&j2se-5_0;JavaxManagementTimer">
		<rdfs:subClassOf rdf:resource="&java;JavaAPIPart"/>
		<rdfs:seeAlso rdf:resource="&j2se-5_0;JavaUtil"/>
		<rdfs:seeAlso rdf:resource="&j2se-5_0;JavaLang"/>
		<rdfs:seeAlso rdf:resource="&j2se-5_0;JavaxManagement"/>
		<rdfs:comment xml:lang="en">Java API part implementing the javax.management.timer package for J2SE 5.0</rdfs:comment>
	</owl:Class>
	<owl:Class rdf:about="&j2se-5_0;JavaxActivity">
		<rdfs:subClassOf rdf:resource="&java;JavaAPIPart"/>
		<rdfs:seeAlso rdf:resource="&j2se-5_0;JavaLang"/>
		<rdfs:seeAlso rdf:resource="&j2se-5_0;JavaRmi"/>
		<rdfs:comment xml:lang="en">Java API part implementing the javax.activity package for J2SE 5.0</rdfs:comment>
	</owl:Class>
	<owl:Class rdf:about="&j2se-5_0;JavaxImageio">
		<owl:equivalentClass rdf:resource="&j2se-1_4;JavaxImageio"/>
		<rdfs:subClassOf rdf:resource="&java;JavaAPIPart"/>
		<rdfs:seeAlso rdf:resource="&j2se-5_0;JavaxImageioStream"/>
		<rdfs:seeAlso rdf:resource="&j2se-5_0;JavaxImageioMetadata"/>
		<rdfs:seeAlso rdf:resource="&j2se-5_0;JavaNet"/>
		<rdfs:seeAlso rdf:resource="&j2se-5_0;JavaIo"/>
		<rdfs:seeAlso rdf:resource="&j2se-5_0;JavaAwtImage"/>
		<rdfs:seeAlso rdf:resource="&j2se-5_0;JavaAwtColor"/>
		<rdfs:seeAlso rdf:resource="&j2se-5_0;JavaAwt"/>
		<rdfs:seeAlso rdf:resource="&j2se-5_0;JavaxImageioSpi"/>
		<rdfs:seeAlso rdf:resource="&j2se-5_0;JavaUtil"/>
		<rdfs:seeAlso rdf:resource="&j2se-5_0;JavaxImageioEvent"/>
		<rdfs:seeAlso rdf:resource="&j2se-5_0;JavaLang"/>
		<rdfs:comment xml:lang="en">Java API part implementing the javax.imageio package for J2SE 5.0</rdfs:comment>
	</owl:Class>
	<owl:Class rdf:about="&j2se-5_0;JavaxImageioMetadata">
		<rdfs:subClassOf rdf:resource="&j2se-1_4;JavaxImageioMetadata"/>
		<rdfs:seeAlso rdf:resource="&j2se-5_0;OrgW3cDom"/>
		<rdfs:seeAlso rdf:resource="&j2se-5_0;JavaUtil"/>
		<rdfs:seeAlso rdf:resource="&j2se-5_0;JavaxImageio"/>
		<rdfs:seeAlso rdf:resource="&j2se-5_0;JavaLang"/>
		<rdfs:comment xml:lang="en">Java API part implementing the javax.imageio.metadata package for J2SE 5.0</rdfs:comment>
	</owl:Class>
	<owl:Class rdf:about="&j2se-5_0;JavaxImageioEvent">
		<owl:equivalentClass rdf:resource="&j2se-1_4;JavaxImageioEvent"/>
		<rdfs:subClassOf rdf:resource="&java;JavaAPIPart"/>
		<rdfs:seeAlso rdf:resource="&j2se-5_0;JavaxImageio"/>
		<rdfs:seeAlso rdf:resource="&j2se-5_0;JavaLang"/>
		<rdfs:seeAlso rdf:resource="&j2se-5_0;JavaAwtImage"/>
		<rdfs:seeAlso rdf:resource="&j2se-5_0;JavaUtil"/>
		<rdfs:comment xml:lang="en">Java API part implementing the javax.imageio.event package for J2SE 5.0</rdfs:comment>
	</owl:Class>
	<owl:Class rdf:about="&j2se-5_0;JavaxImageioPluginsBmp">
		<rdfs:subClassOf rdf:resource="&java;JavaAPIPart"/>
		<rdfs:seeAlso rdf:resource="&j2se-5_0;JavaxImageio"/>
		<rdfs:seeAlso rdf:resource="&j2se-5_0;JavaUtil"/>
		<rdfs:comment xml:lang="en">Java API part implementing the javax.imageio.plugins.bmp package for J2SE 5.0</rdfs:comment>
	</owl:Class>
	<owl:Class rdf:about="&j2se-5_0;JavaxImageioPluginsJpeg">
		<owl:equivalentClass rdf:resource="&j2se-1_4;JavaxImageioPluginsJpeg"/>
		<rdfs:subClassOf rdf:resource="&java;JavaAPIPart"/>
		<rdfs:seeAlso rdf:resource="&j2se-5_0;JavaxImageio"/>
		<rdfs:seeAlso rdf:resource="&j2se-5_0;JavaLang"/>
		<rdfs:seeAlso rdf:resource="&j2se-5_0;JavaUtil"/>
		<rdfs:comment xml:lang="en">Java API part implementing the javax.imageio.plugins.jpeg package for J2SE 5.0</rdfs:comment>
	</owl:Class>
	<owl:Class rdf:about="&j2se-5_0;JavaxImageioStream">
		<owl:equivalentClass rdf:resource="&j2se-1_4;JavaxImageioStream"/>
		<rdfs:subClassOf rdf:resource="&java;JavaAPIPart"/>
		<rdfs:seeAlso rdf:resource="&j2se-5_0;JavaLang"/>
		<rdfs:seeAlso rdf:resource="&j2se-5_0;JavaNio"/>
		<rdfs:seeAlso rdf:resource="&j2se-5_0;JavaIo"/>
		<rdfs:comment xml:lang="en">Java API part implementing the javax.imageio.stream package for J2SE 5.0</rdfs:comment>
	</owl:Class>
	<owl:Class rdf:about="&j2se-5_0;JavaxImageioSpi">
		<owl:equivalentClass rdf:resource="&j2se-1_4;JavaxImageioSpi"/>
		<rdfs:subClassOf rdf:resource="&java;JavaAPIPart"/>
		<rdfs:seeAlso rdf:resource="&j2se-5_0;JavaxImageioStream"/>
		<rdfs:seeAlso rdf:resource="&j2se-5_0;JavaxImageioMetadata"/>
		<rdfs:seeAlso rdf:resource="&j2se-5_0;JavaUtil"/>
		<rdfs:seeAlso rdf:resource="&j2se-5_0;JavaIo"/>
		<rdfs:seeAlso rdf:resource="&j2se-5_0;JavaxImageio"/>
		<rdfs:seeAlso rdf:resource="&j2se-5_0;JavaLang"/>
		<rdfs:seeAlso rdf:resource="&j2se-5_0;JavaAwtImage"/>
		<rdfs:comment xml:lang="en">Java API part implementing the javax.imageio.spi package for J2SE 5.0</rdfs:comment>
	</owl:Class>
	<owl:Class rdf:about="&j2se-5_0;JavaxNaming">
		<rdfs:subClassOf rdf:resource="&j2se-1_4;JavaxNaming"/>
		<rdfs:seeAlso rdf:resource="&j2se-5_0;JavaLang"/>
		<rdfs:seeAlso rdf:resource="&j2se-5_0;JavaUtil"/>
		<rdfs:seeAlso rdf:resource="&j2se-5_0;JavaIo"/>
		<rdfs:comment xml:lang="en">Java API part implementing the javax.naming package for J2SE 5.0</rdfs:comment>
	</owl:Class>
	<owl:Class rdf:about="&j2se-5_0;JavaxNamingDirectory">
		<rdfs:subClassOf rdf:resource="&j2se-1_4;JavaxNamingDirectory"/>
		<rdfs:seeAlso rdf:resource="&j2se-5_0;JavaxNaming"/>
		<rdfs:seeAlso rdf:resource="&j2se-5_0;JavaUtil"/>
		<rdfs:seeAlso rdf:resource="&j2se-5_0;JavaIo"/>
		<rdfs:seeAlso rdf:resource="&j2se-5_0;JavaLang"/>
		<rdfs:comment xml:lang="en">Java API part implementing the javax.naming.directory package for J2SE 5.0</rdfs:comment>
	</owl:Class>
	<owl:Class rdf:about="&j2se-5_0;JavaxNamingEvent">
		<owl:equivalentClass rdf:resource="&j2se-1_4;JavaxNamingEvent"/>
		<rdfs:subClassOf rdf:resource="&java;JavaAPIPart"/>
		<rdfs:seeAlso rdf:resource="&j2se-5_0;JavaxNaming"/>
		<rdfs:seeAlso rdf:resource="&j2se-5_0;JavaxNamingDirectory"/>
		<rdfs:seeAlso rdf:resource="&j2se-5_0;JavaLang"/>
		<rdfs:seeAlso rdf:resource="&j2se-5_0;JavaUtil"/>
		<rdfs:comment xml:lang="en">Java API part implementing the javax.naming.event package for J2SE 5.0</rdfs:comment>
	</owl:Class>
	<owl:Class rdf:about="&j2se-5_0;JavaxNamingLdap">
		<rdfs:subClassOf rdf:resource="&j2se-1_4;JavaxNamingLdap"/>
		<rdfs:seeAlso rdf:resource="&j2se-5_0;JavaxNaming"/>
		<rdfs:seeAlso rdf:resource="&j2se-5_0;JavaUtil"/>
		<rdfs:seeAlso rdf:resource="&j2se-5_0;JavaIo"/>
		<rdfs:seeAlso rdf:resource="&j2se-5_0;JavaxNamingEvent"/>
		<rdfs:seeAlso rdf:resource="&j2se-5_0;JavaxNetSsl"/>
		<rdfs:seeAlso rdf:resource="&j2se-5_0;JavaxNamingDirectory"/>
		<rdfs:seeAlso rdf:resource="&j2se-5_0;JavaLang"/>
		<rdfs:comment xml:lang="en">Java API part implementing the javax.naming.ldap package for J2SE 5.0</rdfs:comment>
	</owl:Class>
	<owl:Class rdf:about="&j2se-5_0;JavaxNamingSpi">
		<owl:equivalentClass rdf:resource="&j2se-1_4;JavaxNamingSpi"/>
		<rdfs:subClassOf rdf:resource="&java;JavaAPIPart"/>
		<rdfs:seeAlso rdf:resource="&j2se-5_0;JavaxNaming"/>
		<rdfs:seeAlso rdf:resource="&j2se-5_0;JavaxNamingDirectory"/>
		<rdfs:seeAlso rdf:resource="&j2se-5_0;JavaLang"/>
		<rdfs:seeAlso rdf:resource="&j2se-5_0;JavaUtil"/>
		<rdfs:seeAlso rdf:resource="&j2se-5_0;JavaIo"/>
		<rdfs:comment xml:lang="en">Java API part implementing the javax.naming.spi package for J2SE 5.0</rdfs:comment>
	</owl:Class>
	<owl:Class rdf:about="&j2se-5_0;JavaxPrint">
		<owl:equivalentClass rdf:resource="&j2se-1_4;JavaxPrint"/>
		<rdfs:subClassOf rdf:resource="&java;JavaAPIPart"/>
		<rdfs:seeAlso rdf:resource="&j2se-5_0;JavaAwt"/>
		<rdfs:seeAlso rdf:resource="&j2se-5_0;JavaNet"/>
		<rdfs:seeAlso rdf:resource="&j2se-5_0;JavaIo"/>
		<rdfs:seeAlso rdf:resource="&j2se-5_0;JavaxPrintAttribute"/>
		<rdfs:seeAlso rdf:resource="&j2se-5_0;JavaLang"/>
		<rdfs:seeAlso rdf:resource="&j2se-5_0;JavaxPrintEvent"/>
		<rdfs:comment xml:lang="en">Java API part implementing the javax.print package for J2SE 5.0</rdfs:comment>
	</owl:Class>
	<owl:Class rdf:about="&j2se-5_0;JavaxPrintAttribute">
		<owl:equivalentClass rdf:resource="&j2se-1_4;JavaxPrintAttribute"/>
		<rdfs:subClassOf rdf:resource="&java;JavaAPIPart"/>
		<rdfs:seeAlso rdf:resource="&j2se-5_0;JavaLang"/>
		<rdfs:seeAlso rdf:resource="&j2se-5_0;JavaUtil"/>
		<rdfs:seeAlso rdf:resource="&j2se-5_0;JavaNet"/>
		<rdfs:seeAlso rdf:resource="&j2se-5_0;JavaIo"/>
		<rdfs:comment xml:lang="en">Java API part implementing the javax.print.attribute package for J2SE 5.0</rdfs:comment>
	</owl:Class>
	<owl:Class rdf:about="&j2se-5_0;JavaxPrintAttributeStandard">
		<rdfs:subClassOf rdf:resource="&j2se-1_4;JavaxPrintAttributeStandard"/>
		<rdfs:seeAlso rdf:resource="&j2se-5_0;JavaNet"/>
		<rdfs:seeAlso rdf:resource="&j2se-5_0;JavaUtil"/>
		<rdfs:seeAlso rdf:resource="&j2se-5_0;JavaxPrintAttribute"/>
		<rdfs:seeAlso rdf:resource="&j2se-5_0;JavaLang"/>
		<rdfs:comment xml:lang="en">Java API part implementing the javax.print.attribute.standard package for J2SE 5.0</rdfs:comment>
	</owl:Class>
	<owl:Class rdf:about="&j2se-5_0;JavaxPrintEvent">
		<owl:equivalentClass rdf:resource="&j2se-1_4;JavaxPrintEvent"/>
		<rdfs:subClassOf rdf:resource="&java;JavaAPIPart"/>
		<rdfs:seeAlso rdf:resource="&j2se-5_0;JavaxPrint"/>
		<rdfs:seeAlso rdf:resource="&j2se-5_0;JavaxPrintAttribute"/>
		<rdfs:seeAlso rdf:resource="&j2se-5_0;JavaLang"/>
		<rdfs:seeAlso rdf:resource="&j2se-5_0;JavaUtil"/>
		<rdfs:comment xml:lang="en">Java API part implementing the javax.print.event package for J2SE 5.0</rdfs:comment>
	</owl:Class>
	<owl:Class rdf:about="&j2se-5_0;JavaxRmi">
		<owl:equivalentClass rdf:resource="&j2se-1_4;JavaxRmi"/>
		<rdfs:subClassOf rdf:resource="&java;JavaAPIPart"/>
		<rdfs:seeAlso rdf:resource="&j2se-5_0;JavaLang"/>
		<rdfs:seeAlso rdf:resource="&j2se-5_0;JavaRmi"/>
		<rdfs:comment xml:lang="en">Java API part implementing the javax.rmi package for J2SE 5.0</rdfs:comment>
	</owl:Class>
	<owl:Class rdf:about="&j2se-5_0;JavaxRmiCORBA">
		<rdfs:subClassOf rdf:resource="&j2se-1_4;JavaxRmiCORBA"/>
		<rdfs:seeAlso rdf:resource="&j2se-5_0;OrgOmgCORBA"/>
		<rdfs:seeAlso rdf:resource="&j2se-5_0;OrgOmgSendingContext"/>
		<rdfs:seeAlso rdf:resource="&j2se-5_0;JavaRmi"/>
		<rdfs:seeAlso rdf:resource="&j2se-5_0;JavaIo"/>
		<rdfs:seeAlso rdf:resource="&j2se-5_0;OrgOmgCORBAPortable"/>
		<rdfs:seeAlso rdf:resource="&j2se-5_0;OrgOmgCORBA_2_3Portable"/>
		<rdfs:seeAlso rdf:resource="&j2se-5_0;JavaLang"/>
		<rdfs:comment xml:lang="en">Java API part implementing the javax.rmi.CORBA package for J2SE 5.0</rdfs:comment>
	</owl:Class>
	<owl:Class rdf:about="&j2se-5_0;JavaxRmiSsl">
		<rdfs:subClassOf rdf:resource="&java;JavaAPIPart"/>
		<rdfs:seeAlso rdf:resource="&j2se-5_0;JavaRmiServer"/>
		<rdfs:seeAlso rdf:resource="&j2se-5_0;JavaLang"/>
		<rdfs:seeAlso rdf:resource="&j2se-5_0;JavaNet"/>
		<rdfs:seeAlso rdf:resource="&j2se-5_0;JavaIo"/>
		<rdfs:comment xml:lang="en">Java API part implementing the javax.rmi.ssl package for J2SE 5.0</rdfs:comment>
	</owl:Class>
	<owl:Class rdf:about="&j2se-5_0;JavaxSoundMidi">
		<rdfs:subClassOf rdf:resource="&java;JavaAPIPart"/>
		<rdfs:seeAlso rdf:resource="&j2se-5_0;JavaNet"/>
		<rdfs:seeAlso rdf:resource="&j2se-5_0;JavaUtil"/>
		<rdfs:seeAlso rdf:resource="&j2se-5_0;JavaIo"/>
		<rdfs:seeAlso rdf:resource="&j2se-5_0;JavaLang"/>
		<rdfs:comment xml:lang="en">Java API part implementing the javax.sound.midi package for J2SE 5.0</rdfs:comment>
	</owl:Class>
	<owl:Class rdf:about="&j2se-5_0;JavaxSoundMidiSpi">
		<owl:equivalentClass rdf:resource="&j2se-1_4;JavaxSoundMidiSpi"/>
		<rdfs:subClassOf rdf:resource="&java;JavaAPIPart"/>
		<rdfs:seeAlso rdf:resource="&j2se-5_0;JavaLang"/>
		<rdfs:seeAlso rdf:resource="&j2se-5_0;JavaxSoundMidi"/>
		<rdfs:seeAlso rdf:resource="&j2se-5_0;JavaNet"/>
		<rdfs:seeAlso rdf:resource="&j2se-5_0;JavaIo"/>
		<rdfs:comment xml:lang="en">Java API part implementing the javax.sound.midi.spi package for J2SE 5.0</rdfs:comment>
	</owl:Class>
	<owl:Class rdf:about="&j2se-5_0;JavaxSoundSampled">
		<rdfs:subClassOf rdf:resource="&j2se-1_4;JavaxSoundSampled"/>
		<rdfs:seeAlso rdf:resource="&j2se-5_0;JavaSecurity"/>
		<rdfs:seeAlso rdf:resource="&j2se-5_0;JavaNet"/>
		<rdfs:seeAlso rdf:resource="&j2se-5_0;JavaUtil"/>
		<rdfs:seeAlso rdf:resource="&j2se-5_0;JavaIo"/>
		<rdfs:seeAlso rdf:resource="&j2se-5_0;JavaLang"/>
		<rdfs:comment xml:lang="en">Java API part implementing the javax.sound.sampled package for J2SE 5.0</rdfs:comment>
	</owl:Class>
	<owl:Class rdf:about="&j2se-5_0;JavaxSoundSampledSpi">
		<owl:equivalentClass rdf:resource="&j2se-1_4;JavaxSoundSampledSpi"/>
		<rdfs:subClassOf rdf:resource="&java;JavaAPIPart"/>
		<rdfs:seeAlso rdf:resource="&j2se-5_0;JavaNet"/>
		<rdfs:seeAlso rdf:resource="&j2se-5_0;JavaIo"/>
		<rdfs:seeAlso rdf:resource="&j2se-5_0;JavaxSoundSampled"/>
		<rdfs:seeAlso rdf:resource="&j2se-5_0;JavaLang"/>
		<rdfs:comment xml:lang="en">Java API part implementing the javax.sound.sampled.spi package for J2SE 5.0</rdfs:comment>
	</owl:Class>
	<owl:Class rdf:about="&j2se-5_0;JavaxSql">
		<owl:equivalentClass rdf:resource="&j2se-1_4;JavaxSql"/>
		<rdfs:subClassOf rdf:resource="&java;JavaAPIPart"/>
		<rdfs:seeAlso rdf:resource="&j2se-5_0;JavaMath"/>
		<rdfs:seeAlso rdf:resource="&j2se-5_0;JavaSql"/>
		<rdfs:seeAlso rdf:resource="&j2se-5_0;JavaUtil"/>
		<rdfs:seeAlso rdf:resource="&j2se-5_0;JavaIo"/>
		<rdfs:seeAlso rdf:resource="&j2se-5_0;JavaxTransactionXa"/>
		<rdfs:seeAlso rdf:resource="&j2se-5_0;JavaLang"/>
		<rdfs:comment xml:lang="en">Java API part implementing the javax.sql package for J2SE 5.0</rdfs:comment>
	</owl:Class>
	<owl:Class rdf:about="&j2se-5_0;JavaxSqlRowset">
		<rdfs:subClassOf rdf:resource="&java;JavaAPIPart"/>
		<rdfs:seeAlso rdf:resource="&j2se-5_0;JavaMath"/>
		<rdfs:seeAlso rdf:resource="&j2se-5_0;JavaSql"/>
		<rdfs:seeAlso rdf:resource="&j2se-5_0;JavaIo"/>
		<rdfs:seeAlso rdf:resource="&j2se-5_0;JavaxSqlRowsetSpi"/>
		<rdfs:seeAlso rdf:resource="&j2se-5_0;JavaxSql"/>
		<rdfs:seeAlso rdf:resource="&j2se-5_0;JavaUtil"/>
		<rdfs:seeAlso rdf:resource="&j2se-5_0;JavaLang"/>
		<rdfs:comment xml:lang="en">Java API part implementing the javax.sql.rowset package for J2SE 5.0</rdfs:comment>
	</owl:Class>
	<owl:Class rdf:about="&j2se-5_0;JavaxSqlRowsetSpi">
		<rdfs:subClassOf rdf:resource="&java;JavaAPIPart"/>
		<rdfs:seeAlso rdf:resource="&j2se-5_0;JavaxNaming"/>
		<rdfs:seeAlso rdf:resource="&j2se-5_0;JavaSql"/>
		<rdfs:seeAlso rdf:resource="&j2se-5_0;JavaxSql"/>
		<rdfs:seeAlso rdf:resource="&j2se-5_0;JavaUtil"/>
		<rdfs:seeAlso rdf:resource="&j2se-5_0;JavaIo"/>
		<rdfs:seeAlso rdf:resource="&j2se-5_0;JavaxSqlRowset"/>
		<rdfs:seeAlso rdf:resource="&j2se-5_0;JavaLang"/>
		<rdfs:seeAlso rdf:resource="&j2se-5_0;JavaUtilLogging"/>
		<rdfs:comment xml:lang="en">Java API part implementing the javax.sql.rowset.spi package for J2SE 5.0</rdfs:comment>
	</owl:Class>
	<owl:Class rdf:about="&j2se-5_0;JavaxSqlRowsetSerial">
		<rdfs:subClassOf rdf:resource="&java;JavaAPIPart"/>
		<rdfs:seeAlso rdf:resource="&j2se-5_0;JavaMath"/>
		<rdfs:seeAlso rdf:resource="&j2se-5_0;JavaSql"/>
		<rdfs:seeAlso rdf:resource="&j2se-5_0;JavaNet"/>
		<rdfs:seeAlso rdf:resource="&j2se-5_0;JavaIo"/>
		<rdfs:seeAlso rdf:resource="&j2se-5_0;JavaUtil"/>
		<rdfs:seeAlso rdf:resource="&j2se-5_0;JavaLang"/>
		<rdfs:comment xml:lang="en">Java API part implementing the javax.sql.rowset.serial package for J2SE 5.0</rdfs:comment>
	</owl:Class>
	<owl:Class rdf:about="&j2se-5_0;JavaxTransaction">
		<owl:equivalentClass rdf:resource="&j2se-1_4;JavaxTransaction"/>
		<rdfs:subClassOf rdf:resource="&java;JavaAPIPart"/>
		<rdfs:seeAlso rdf:resource="&j2se-5_0;JavaLang"/>
		<rdfs:seeAlso rdf:resource="&j2se-5_0;JavaRmi"/>
		<rdfs:comment xml:lang="en">Java API part implementing the javax.transaction package for J2SE 5.0</rdfs:comment>
	</owl:Class>
	<owl:Class rdf:about="&j2se-5_0;JavaxTransactionXa">
		<owl:equivalentClass rdf:resource="&j2se-1_4;JavaxTransactionXa"/>
		<rdfs:subClassOf rdf:resource="&java;JavaAPIPart"/>
		<rdfs:seeAlso rdf:resource="&j2se-5_0;JavaLang"/>
		<rdfs:comment xml:lang="en">Java API part implementing the javax.transaction.xa package for J2SE 5.0</rdfs:comment>
	</owl:Class>
	<owl:Class rdf:about="&j2se-5_0;JavaxXml">
		<rdfs:subClassOf rdf:resource="&java;JavaAPIPart"/>
		<rdfs:seeAlso rdf:resource="&j2se-5_0;JavaLang"/>
		<rdfs:comment xml:lang="en">Java API part implementing the javax.xml package for J2SE 5.0</rdfs:comment>
	</owl:Class>
	<owl:Class rdf:about="&j2se-5_0;JavaxXmlDatatype">
		<rdfs:subClassOf rdf:resource="&java;JavaAPIPart"/>
		<rdfs:seeAlso rdf:resource="&j2se-5_0;JavaMath"/>
		<rdfs:seeAlso rdf:resource="&j2se-5_0;JavaUtil"/>
		<rdfs:seeAlso rdf:resource="&j2se-5_0;JavaLang"/>
		<rdfs:seeAlso rdf:resource="&j2se-5_0;JavaxXmlNamespace"/>
		<rdfs:comment xml:lang="en">Java API part implementing the javax.xml.datatype package for J2SE 5.0</rdfs:comment>
	</owl:Class>
	<owl:Class rdf:about="&j2se-5_0;JavaxXmlNamespace">
		<rdfs:subClassOf rdf:resource="&java;JavaAPIPart"/>
		<rdfs:seeAlso rdf:resource="&j2se-5_0;JavaLang"/>
		<rdfs:seeAlso rdf:resource="&j2se-5_0;JavaUtil"/>
		<rdfs:seeAlso rdf:resource="&j2se-5_0;JavaIo"/>
		<rdfs:comment xml:lang="en">Java API part implementing the javax.xml.namespace package for J2SE 5.0</rdfs:comment>
	</owl:Class>
	<owl:Class rdf:about="&j2se-5_0;JavaxXmlTransform">
		<rdfs:subClassOf rdf:resource="&j2se-1_4;JavaxXmlTransform"/>
		<rdfs:seeAlso rdf:resource="&j2se-5_0;JavaLang"/>
		<rdfs:seeAlso rdf:resource="&j2se-5_0;JavaUtil"/>
		<rdfs:seeAlso rdf:resource="&j2se-5_0;JavaIo"/>
		<rdfs:comment xml:lang="en">Java API part implementing the javax.xml.transform package for J2SE 5.0</rdfs:comment>
	</owl:Class>
	<owl:Class rdf:about="&j2se-5_0;JavaxXmlTransformDom">
		<rdfs:subClassOf rdf:resource="&j2se-1_4;JavaxXmlTransformDom"/>
		<rdfs:seeAlso rdf:resource="&j2se-5_0;OrgW3cDom"/>
		<rdfs:seeAlso rdf:resource="&j2se-5_0;JavaxXmlTransform"/>
		<rdfs:seeAlso rdf:resource="&j2se-5_0;JavaLang"/>
		<rdfs:comment xml:lang="en">Java API part implementing the javax.xml.transform.dom package for J2SE 5.0</rdfs:comment>
	</owl:Class>
	<owl:Class rdf:about="&j2se-5_0;JavaxXmlTransformSax">
		<rdfs:subClassOf rdf:resource="&j2se-1_4;JavaxXmlTransformSax"/>
		<rdfs:seeAlso rdf:resource="&j2se-5_0;OrgXmlSax"/>
		<rdfs:seeAlso rdf:resource="&j2se-5_0;OrgXmlSaxExt"/>
		<rdfs:seeAlso rdf:resource="&j2se-5_0;JavaxXmlTransform"/>
		<rdfs:seeAlso rdf:resource="&j2se-5_0;JavaLang"/>
		<rdfs:comment xml:lang="en">Java API part implementing the javax.xml.transform.sax package for J2SE 5.0</rdfs:comment>
	</owl:Class>
	<owl:Class rdf:about="&j2se-5_0;JavaxXmlTransformStream">
		<owl:equivalentClass rdf:resource="&j2se-1_4;JavaxXmlTransformStream"/>
		<rdfs:subClassOf rdf:resource="&java;JavaAPIPart"/>
		<rdfs:seeAlso rdf:resource="&j2se-5_0;JavaxXmlTransform"/>
		<rdfs:seeAlso rdf:resource="&j2se-5_0;JavaLang"/>
		<rdfs:seeAlso rdf:resource="&j2se-5_0;JavaIo"/>
		<rdfs:comment xml:lang="en">Java API part implementing the javax.xml.transform.stream package for J2SE 5.0</rdfs:comment>
	</owl:Class>
	<owl:Class rdf:about="&j2se-5_0;JavaxXmlValidation">
		<rdfs:subClassOf rdf:resource="&java;JavaAPIPart"/>
		<rdfs:seeAlso rdf:resource="&j2se-5_0;OrgXmlSax"/>
		<rdfs:seeAlso rdf:resource="&j2se-5_0;OrgW3cDom"/>
		<rdfs:seeAlso rdf:resource="&j2se-5_0;OrgW3cDomLs"/>
		<rdfs:seeAlso rdf:resource="&j2se-5_0;JavaxXmlTransform"/>
		<rdfs:seeAlso rdf:resource="&j2se-5_0;JavaLang"/>
		<rdfs:seeAlso rdf:resource="&j2se-5_0;JavaNet"/>
		<rdfs:seeAlso rdf:resource="&j2se-5_0;JavaIo"/>
		<rdfs:comment xml:lang="en">Java API part implementing the javax.xml.validation package for J2SE 5.0</rdfs:comment>
	</owl:Class>
	<owl:Class rdf:about="&j2se-5_0;JavaxXmlXpath">
		<rdfs:subClassOf rdf:resource="&java;JavaAPIPart"/>
		<rdfs:seeAlso rdf:resource="&j2se-5_0;OrgXmlSax"/>
		<rdfs:seeAlso rdf:resource="&j2se-5_0;JavaLang"/>
		<rdfs:seeAlso rdf:resource="&j2se-5_0;JavaUtil"/>
		<rdfs:seeAlso rdf:resource="&j2se-5_0;JavaIo"/>
		<rdfs:seeAlso rdf:resource="&j2se-5_0;JavaxXmlNamespace"/>
		<rdfs:comment xml:lang="en">Java API part implementing the javax.xml.xpath package for J2SE 5.0</rdfs:comment>
	</owl:Class>
	<owl:Class rdf:about="&j2se-5_0;JavaxXmlParsers">
		<rdfs:subClassOf rdf:resource="&j2se-1_4;JavaxXmlParsers"/>
		<rdfs:seeAlso rdf:resource="&j2se-5_0;OrgXmlSax"/>
		<rdfs:seeAlso rdf:resource="&j2se-5_0;JavaxXmlValidation"/>
		<rdfs:seeAlso rdf:resource="&j2se-5_0;OrgW3cDom"/>
		<rdfs:seeAlso rdf:resource="&j2se-5_0;JavaIo"/>
		<rdfs:seeAlso rdf:resource="&j2se-5_0;JavaLang"/>
		<rdfs:seeAlso rdf:resource="&j2se-5_0;OrgXmlSaxHelpers"/>
		<rdfs:comment xml:lang="en">Java API part implementing the javax.xml.parsers package for J2SE 5.0</rdfs:comment>
	</owl:Class>
	<owl:Class rdf:about="&j2se-5_0;JavaLang">
		<rdfs:subClassOf rdf:resource="&j2se-1_4;JavaLang"/>
		<rdfs:seeAlso rdf:resource="&j2se-5_0;JavaNet"/>
		<rdfs:seeAlso rdf:resource="&j2se-5_0;JavaIo"/>
		<rdfs:seeAlso rdf:resource="&j2se-5_0;JavaLangReflect"/>
		<rdfs:seeAlso rdf:resource="&j2se-5_0;JavaLangAnnotation"/>
		<rdfs:seeAlso rdf:resource="&j2se-5_0;JavaSecurity"/>
		<rdfs:seeAlso rdf:resource="&j2se-5_0;JavaUtil"/>
		<rdfs:seeAlso rdf:resource="&j2se-5_0;JavaNio"/>
		<rdfs:seeAlso rdf:resource="&j2se-5_0;JavaNioChannels"/>
		<rdfs:comment xml:lang="en">Java API part implementing the java.lang package for J2SE 5.0</rdfs:comment>
	</owl:Class>
	<owl:Class rdf:about="&j2se-5_0;JavaLangReflect">
		<rdfs:subClassOf rdf:resource="&j2se-1_4;JavaLangReflect"/>
		<rdfs:seeAlso rdf:resource="&j2se-5_0;JavaLangAnnotation"/>
		<rdfs:seeAlso rdf:resource="&j2se-5_0;JavaSecurity"/>
		<rdfs:seeAlso rdf:resource="&j2se-5_0;JavaLang"/>
		<rdfs:seeAlso rdf:resource="&j2se-5_0;JavaIo"/>
		<rdfs:comment xml:lang="en">Java API part implementing the java.lang.reflect package for J2SE 5.0</rdfs:comment>
	</owl:Class>
	<owl:Class rdf:about="&j2se-5_0;JavaLangAnnotation">
		<rdfs:subClassOf rdf:resource="&java;JavaAPIPart"/>
		<rdfs:seeAlso rdf:resource="&j2se-5_0;JavaLangReflect"/>
		<rdfs:seeAlso rdf:resource="&j2se-5_0;JavaLang"/>
		<rdfs:comment xml:lang="en">Java API part implementing the java.lang.annotation package for J2SE 5.0</rdfs:comment>
	</owl:Class>
	<owl:Class rdf:about="&j2se-5_0;JavaLangInstrument">
		<rdfs:subClassOf rdf:resource="&java;JavaAPIPart"/>
		<rdfs:seeAlso rdf:resource="&j2se-5_0;JavaSecurity"/>
		<rdfs:seeAlso rdf:resource="&j2se-5_0;JavaLang"/>
		<rdfs:comment xml:lang="en">Java API part implementing the java.lang.instrument package for J2SE 5.0</rdfs:comment>
	</owl:Class>
	<owl:Class rdf:about="&j2se-5_0;JavaLangManagement">
		<rdfs:subClassOf rdf:resource="&java;JavaAPIPart"/>
		<rdfs:seeAlso rdf:resource="&j2se-5_0;JavaSecurity"/>
		<rdfs:seeAlso rdf:resource="&j2se-5_0;JavaxManagementOpenmbean"/>
		<rdfs:seeAlso rdf:resource="&j2se-5_0;JavaLang"/>
		<rdfs:seeAlso rdf:resource="&j2se-5_0;JavaxManagement"/>
		<rdfs:seeAlso rdf:resource="&j2se-5_0;JavaUtil"/>
		<rdfs:comment xml:lang="en">Java API part implementing the java.lang.management package for J2SE 5.0</rdfs:comment>
	</owl:Class>
	<owl:Class rdf:about="&j2se-5_0;JavaLangRef">
		<owl:equivalentClass rdf:resource="&j2se-1_4;JavaLangRef"/>
		<rdfs:subClassOf rdf:resource="&java;JavaAPIPart"/>
		<rdfs:seeAlso rdf:resource="&j2se-5_0;JavaLang"/>
		<rdfs:comment xml:lang="en">Java API part implementing the java.lang.ref package for J2SE 5.0</rdfs:comment>
	</owl:Class>
	<owl:Class rdf:about="&j2se-5_0;JavaSecurity">
		<rdfs:subClassOf rdf:resource="&j2se-1_4;JavaSecurity"/>
		<rdfs:seeAlso rdf:resource="&j2se-5_0;JavaNet"/>
		<rdfs:seeAlso rdf:resource="&j2se-5_0;JavaIo"/>
		<rdfs:seeAlso rdf:resource="&j2se-5_0;JavaxSecurityAuth"/>
		<rdfs:seeAlso rdf:resource="&j2se-5_0;JavaSecuritySpec"/>
		<rdfs:seeAlso rdf:resource="&j2se-5_0;JavaxSecurityAuthCallback"/>
		<rdfs:seeAlso rdf:resource="&j2se-5_0;JavaxCrypto"/>
		<rdfs:seeAlso rdf:resource="&j2se-5_0;JavaUtil"/>
		<rdfs:seeAlso rdf:resource="&j2se-5_0;JavaNio"/>
		<rdfs:seeAlso rdf:resource="&j2se-5_0;JavaLang"/>
		<rdfs:seeAlso rdf:resource="&j2se-5_0;JavaSecurityCert"/>
		<rdfs:comment xml:lang="en">Java API part implementing the java.security package for J2SE 5.0</rdfs:comment>
	</owl:Class>
	<owl:Class rdf:about="&j2se-5_0;JavaSecuritySpec">
		<rdfs:subClassOf rdf:resource="&j2se-1_4;JavaSecuritySpec"/>
		<rdfs:seeAlso rdf:resource="&j2se-5_0;JavaSecurityInterfaces"/>
		<rdfs:seeAlso rdf:resource="&j2se-5_0;JavaMath"/>
		<rdfs:seeAlso rdf:resource="&j2se-5_0;JavaSecurity"/>
		<rdfs:seeAlso rdf:resource="&j2se-5_0;JavaLang"/>
		<rdfs:comment xml:lang="en">Java API part implementing the java.security.spec package for J2SE 5.0</rdfs:comment>
	</owl:Class>
	<owl:Class rdf:about="&j2se-5_0;JavaSecurityCert">
		<rdfs:subClassOf rdf:resource="&java;JavaAPIPart"/>
		<rdfs:seeAlso rdf:resource="&j2se-5_0;JavaMath"/>
		<rdfs:seeAlso rdf:resource="&j2se-5_0;JavaSecurity"/>
		<rdfs:seeAlso rdf:resource="&j2se-5_0;JavaUtil"/>
		<rdfs:seeAlso rdf:resource="&j2se-5_0;JavaIo"/>
		<rdfs:seeAlso rdf:resource="&j2se-5_0;JavaxSecurityAuthX500"/>
		<rdfs:seeAlso rdf:resource="&j2se-5_0;JavaLang"/>
		<rdfs:comment xml:lang="en">Java API part implementing the java.security.cert package for J2SE 5.0</rdfs:comment>
	</owl:Class>
	<owl:Class rdf:about="&j2se-5_0;JavaSecurityAcl">
		<owl:equivalentClass rdf:resource="&j2se-1_4;JavaSecurityAcl"/>
		<rdfs:subClassOf rdf:resource="&java;JavaAPIPart"/>
		<rdfs:seeAlso rdf:resource="&j2se-5_0;JavaSecurity"/>
		<rdfs:seeAlso rdf:resource="&j2se-5_0;JavaLang"/>
		<rdfs:seeAlso rdf:resource="&j2se-5_0;JavaUtil"/>
		<rdfs:comment xml:lang="en">Java API part implementing the java.security.acl package for J2SE 5.0</rdfs:comment>
	</owl:Class>
	<owl:Class rdf:about="&j2se-5_0;JavaSecurityInterfaces">
		<rdfs:subClassOf rdf:resource="&j2se-1_4;JavaSecurityInterfaces"/>
		<rdfs:seeAlso rdf:resource="&j2se-5_0;JavaSecuritySpec"/>
		<rdfs:seeAlso rdf:resource="&j2se-5_0;JavaMath"/>
		<rdfs:seeAlso rdf:resource="&j2se-5_0;JavaSecurity"/>
		<rdfs:comment xml:lang="en">Java API part implementing the java.security.interfaces package for J2SE 5.0</rdfs:comment>
	</owl:Class>
	<owl:Class rdf:about="&j2se-5_0;JavaMath">
		<rdfs:subClassOf rdf:resource="&j2se-1_4;JavaMath"/>
		<rdfs:seeAlso rdf:resource="&j2se-5_0;JavaLang"/>
		<rdfs:seeAlso rdf:resource="&j2se-5_0;JavaUtil"/>
		<rdfs:seeAlso rdf:resource="&j2se-5_0;JavaIo"/>
		<rdfs:comment xml:lang="en">Java API part implementing the java.math package for J2SE 5.0</rdfs:comment>
	</owl:Class>
	<owl:Class rdf:about="&j2se-5_0;JavaNio">
		<rdfs:subClassOf rdf:resource="&j2se-1_4;JavaNio"/>
		<rdfs:seeAlso rdf:resource="&j2se-5_0;JavaLang"/>
		<rdfs:comment xml:lang="en">Java API part implementing the java.nio package for J2SE 5.0</rdfs:comment>
	</owl:Class>
	<owl:Class rdf:about="&j2se-5_0;JavaNioChannels">
		<rdfs:subClassOf rdf:resource="&j2se-1_4;JavaNioChannels"/>
		<rdfs:seeAlso rdf:resource="&j2se-5_0;JavaUtil"/>
		<rdfs:seeAlso rdf:resource="&j2se-5_0;JavaNet"/>
		<rdfs:seeAlso rdf:resource="&j2se-5_0;JavaIo"/>
		<rdfs:seeAlso rdf:resource="&j2se-5_0;JavaNioCharset"/>
		<rdfs:seeAlso rdf:resource="&j2se-5_0;JavaNio"/>
		<rdfs:seeAlso rdf:resource="&j2se-5_0;JavaLang"/>
		<rdfs:seeAlso rdf:resource="&j2se-5_0;JavaNioChannelsSpi"/>
		<rdfs:comment xml:lang="en">Java API part implementing the java.nio.channels package for J2SE 5.0</rdfs:comment>
	</owl:Class>
	<owl:Class rdf:about="&j2se-5_0;JavaNioChannelsSpi">
		<rdfs:subClassOf rdf:resource="&j2se-1_4;JavaNioChannelsSpi"/>
		<rdfs:seeAlso rdf:resource="&j2se-5_0;JavaLang"/>
		<rdfs:seeAlso rdf:resource="&j2se-5_0;JavaNioChannels"/>
		<rdfs:seeAlso rdf:resource="&j2se-5_0;JavaUtil"/>
		<rdfs:comment xml:lang="en">Java API part implementing the java.nio.channels.spi package for J2SE 5.0</rdfs:comment>
	</owl:Class>
	<owl:Class rdf:about="&j2se-5_0;JavaNioCharset">
		<rdfs:subClassOf rdf:resource="&j2se-1_4;JavaNioCharset"/>
		<rdfs:seeAlso rdf:resource="&j2se-5_0;JavaUtil"/>
		<rdfs:seeAlso rdf:resource="&j2se-5_0;JavaIo"/>
		<rdfs:seeAlso rdf:resource="&j2se-5_0;JavaNio"/>
		<rdfs:seeAlso rdf:resource="&j2se-5_0;JavaLang"/>
		<rdfs:comment xml:lang="en">Java API part implementing the java.nio.charset package for J2SE 5.0</rdfs:comment>
	</owl:Class>
	<owl:Class rdf:about="&j2se-5_0;JavaNioCharsetSpi">
		<owl:equivalentClass rdf:resource="&j2se-1_4;JavaNioCharsetSpi"/>
		<rdfs:subClassOf rdf:resource="&java;JavaAPIPart"/>
		<rdfs:seeAlso rdf:resource="&j2se-5_0;JavaNioCharset"/>
		<rdfs:seeAlso rdf:resource="&j2se-5_0;JavaLang"/>
		<rdfs:seeAlso rdf:resource="&j2se-5_0;JavaUtil"/>
		<rdfs:comment xml:lang="en">Java API part implementing the java.nio.charset.spi package for J2SE 5.0</rdfs:comment>
	</owl:Class>
	<owl:Class rdf:about="&j2se-5_0;JavaIo">
		<rdfs:subClassOf rdf:resource="&j2se-1_4;JavaIo"/>
		<rdfs:seeAlso rdf:resource="&j2se-5_0;JavaSecurity"/>
		<rdfs:seeAlso rdf:resource="&j2se-5_0;JavaUtil"/>
		<rdfs:seeAlso rdf:resource="&j2se-5_0;JavaNet"/>
		<rdfs:seeAlso rdf:resource="&j2se-5_0;JavaNioCharset"/>
		<rdfs:seeAlso rdf:resource="&j2se-5_0;JavaNio"/>
		<rdfs:seeAlso rdf:resource="&j2se-5_0;JavaLang"/>
		<rdfs:seeAlso rdf:resource="&j2se-5_0;JavaNioChannels"/>
		<rdfs:comment xml:lang="en">Java API part implementing the java.io package for J2SE 5.0</rdfs:comment>
	</owl:Class>
	<owl:Class rdf:about="&j2se-5_0;JavaNet">
		<rdfs:subClassOf rdf:resource="&j2se-1_4;JavaNet"/>
		<rdfs:seeAlso rdf:resource="&j2se-5_0;JavaIo"/>
		<rdfs:seeAlso rdf:resource="&j2se-5_0;JavaUtilJar"/>
		<rdfs:seeAlso rdf:resource="&j2se-5_0;JavaSecurity"/>
		<rdfs:seeAlso rdf:resource="&j2se-5_0;JavaUtil"/>
		<rdfs:seeAlso rdf:resource="&j2se-5_0;JavaLang"/>
		<rdfs:seeAlso rdf:resource="&j2se-5_0;JavaNioChannels"/>
		<rdfs:comment xml:lang="en">Java API part implementing the java.net package for J2SE 5.0</rdfs:comment>
	</owl:Class>
	<owl:Class rdf:about="&j2se-5_0;JavaUtil">
		<rdfs:subClassOf rdf:resource="&j2se-1_4;JavaUtil"/>
		<rdfs:seeAlso rdf:resource="&j2se-5_0;JavaMath"/>
		<rdfs:seeAlso rdf:resource="&j2se-5_0;JavaIo"/>
		<rdfs:seeAlso rdf:resource="&j2se-5_0;JavaSecurity"/>
		<rdfs:seeAlso rdf:resource="&j2se-5_0;JavaUtilRegex"/>
		<rdfs:seeAlso rdf:resource="&j2se-5_0;JavaLang"/>
		<rdfs:seeAlso rdf:resource="&j2se-5_0;JavaNioChannels"/>
		<rdfs:comment xml:lang="en">Java API part implementing the java.util package for J2SE 5.0</rdfs:comment>
	</owl:Class>
	<owl:Class rdf:about="&j2se-5_0;JavaUtilRegex">
		<rdfs:subClassOf rdf:resource="&j2se-1_4;JavaUtilRegex"/>
		<rdfs:seeAlso rdf:resource="&j2se-5_0;JavaLang"/>
		<rdfs:seeAlso rdf:resource="&j2se-5_0;JavaIo"/>
		<rdfs:comment xml:lang="en">Java API part implementing the java.util.regex package for J2SE 5.0</rdfs:comment>
	</owl:Class>
	<owl:Class rdf:about="&j2se-5_0;JavaUtilConcurrent">
		<rdfs:subClassOf rdf:resource="&java;JavaAPIPart"/>
		<rdfs:seeAlso rdf:resource="&j2se-5_0;JavaIo"/>
		<rdfs:seeAlso rdf:resource="&j2se-5_0;JavaSecurity"/>
		<rdfs:seeAlso rdf:resource="&j2se-5_0;JavaUtil"/>
		<rdfs:seeAlso rdf:resource="&j2se-5_0;JavaLang"/>
		<rdfs:comment xml:lang="en">Java API part implementing the java.util.concurrent package for J2SE 5.0</rdfs:comment>
	</owl:Class>
	<owl:Class rdf:about="&j2se-5_0;JavaUtilConcurrentAtomic">
		<rdfs:subClassOf rdf:resource="&java;JavaAPIPart"/>
		<rdfs:seeAlso rdf:resource="&j2se-5_0;JavaLang"/>
		<rdfs:seeAlso rdf:resource="&j2se-5_0;JavaIo"/>
		<rdfs:comment xml:lang="en">Java API part implementing the java.util.concurrent.atomic package for J2SE 5.0</rdfs:comment>
	</owl:Class>
	<owl:Class rdf:about="&j2se-5_0;JavaUtilConcurrentLocks">
		<rdfs:subClassOf rdf:resource="&java;JavaAPIPart"/>
		<rdfs:seeAlso rdf:resource="&j2se-5_0;JavaLang"/>
		<rdfs:seeAlso rdf:resource="&j2se-5_0;JavaUtil"/>
		<rdfs:seeAlso rdf:resource="&j2se-5_0;JavaIo"/>
		<rdfs:seeAlso rdf:resource="&j2se-5_0;JavaUtilConcurrent"/>
		<rdfs:comment xml:lang="en">Java API part implementing the java.util.concurrent.locks package for J2SE 5.0</rdfs:comment>
	</owl:Class>
	<owl:Class rdf:about="&j2se-5_0;JavaUtilJar">
		<rdfs:subClassOf rdf:resource="&j2se-1_4;JavaUtilJar"/>
		<rdfs:seeAlso rdf:resource="&j2se-5_0;JavaUtilZip"/>
		<rdfs:seeAlso rdf:resource="&j2se-5_0;JavaUtil"/>
		<rdfs:seeAlso rdf:resource="&j2se-5_0;JavaIo"/>
		<rdfs:seeAlso rdf:resource="&j2se-5_0;JavaLang"/>
		<rdfs:seeAlso rdf:resource="&j2se-5_0;JavaBeans"/>
		<rdfs:comment xml:lang="en">Java API part implementing the java.util.jar package for J2SE 5.0</rdfs:comment>
	</owl:Class>
	<owl:Class rdf:about="&j2se-5_0;JavaUtilZip">
		<rdfs:subClassOf rdf:resource="&j2se-1_4;JavaUtilZip"/>
		<rdfs:seeAlso rdf:resource="&j2se-5_0;JavaLang"/>
		<rdfs:seeAlso rdf:resource="&j2se-5_0;JavaUtil"/>
		<rdfs:seeAlso rdf:resource="&j2se-5_0;JavaIo"/>
		<rdfs:comment xml:lang="en">Java API part implementing the java.util.zip package for J2SE 5.0</rdfs:comment>
	</owl:Class>
	<owl:Class rdf:about="&j2se-5_0;JavaUtilLogging">
		<rdfs:subClassOf rdf:resource="&j2se-1_4;JavaUtilLogging"/>
		<rdfs:seeAlso rdf:resource="&j2se-5_0;JavaSecurity"/>
		<rdfs:seeAlso rdf:resource="&j2se-5_0;JavaUtil"/>
		<rdfs:seeAlso rdf:resource="&j2se-5_0;JavaIo"/>
		<rdfs:seeAlso rdf:resource="&j2se-5_0;JavaLang"/>
		<rdfs:seeAlso rdf:resource="&j2se-5_0;JavaBeans"/>
		<rdfs:comment xml:lang="en">Java API part implementing the java.util.logging package for J2SE 5.0</rdfs:comment>
	</owl:Class>
	<owl:Class rdf:about="&j2se-5_0;JavaUtilPrefs">
		<owl:equivalentClass rdf:resource="&j2se-1_4;JavaUtilPrefs"/>
		<rdfs:subClassOf rdf:resource="&java;JavaAPIPart"/>
		<rdfs:seeAlso rdf:resource="&j2se-5_0;JavaLang"/>
		<rdfs:seeAlso rdf:resource="&j2se-5_0;JavaUtil"/>
		<rdfs:seeAlso rdf:resource="&j2se-5_0;JavaIo"/>
		<rdfs:comment xml:lang="en">Java API part implementing the java.util.prefs package for J2SE 5.0</rdfs:comment>
	</owl:Class>
	<owl:Class rdf:about="&j2se-5_0;JavaApplet">
		<rdfs:subClassOf rdf:resource="&j2se-1_4;JavaApplet"/>
		<rdfs:seeAlso rdf:resource="&j2se-5_0;JavaAwt"/>
		<rdfs:seeAlso rdf:resource="&j2se-5_0;JavaxAccessibility"/>
		<rdfs:seeAlso rdf:resource="&j2se-5_0;JavaNet"/>
		<rdfs:seeAlso rdf:resource="&j2se-5_0;JavaUtil"/>
		<rdfs:seeAlso rdf:resource="&j2se-5_0;JavaIo"/>
		<rdfs:seeAlso rdf:resource="&j2se-5_0;JavaLang"/>
		<rdfs:comment xml:lang="en">Java API part implementing the java.applet package for J2SE 5.0</rdfs:comment>
	</owl:Class>
	<owl:Class rdf:about="&j2se-5_0;JavaAwt">
		<rdfs:subClassOf rdf:resource="&j2se-1_4;JavaAwt"/>
		<rdfs:seeAlso rdf:resource="&j2se-5_0;JavaAwtDatatransfer"/>
		<rdfs:seeAlso rdf:resource="&j2se-5_0;JavaNet"/>
		<rdfs:seeAlso rdf:resource="&j2se-5_0;JavaxSwingText"/>
		<rdfs:seeAlso rdf:resource="&j2se-5_0;JavaAwtColor"/>
		<rdfs:seeAlso rdf:resource="&j2se-5_0;JavaAwtEvent"/>
		<rdfs:seeAlso rdf:resource="&j2se-5_0;JavaAwtFont"/>
		<rdfs:seeAlso rdf:resource="&j2se-5_0;JavaAwtGeom"/>
		<rdfs:seeAlso rdf:resource="&j2se-5_0;JavaUtil"/>
		<rdfs:seeAlso rdf:resource="&j2se-5_0;JavaLang"/>
		<rdfs:seeAlso rdf:resource="&j2se-5_0;JavaAwtDnd"/>
		<rdfs:seeAlso rdf:resource="&j2se-5_0;JavaSecurity"/>
		<rdfs:seeAlso rdf:resource="&j2se-5_0;JavaBeans"/>
		<rdfs:seeAlso rdf:resource="&j2se-5_0;JavaxAccessibility"/>
		<rdfs:seeAlso rdf:resource="&j2se-5_0;JavaIo"/>
		<rdfs:seeAlso rdf:resource="&j2se-5_0;JavaAwtImage"/>
		<rdfs:seeAlso rdf:resource="&j2se-5_0;JavaAwtImageRenderable"/>
		<rdfs:seeAlso rdf:resource="&j2se-5_0;JavaText"/>
		<rdfs:seeAlso rdf:resource="&j2se-5_0;JavaAwtIm"/>
		<rdfs:comment xml:lang="en">Java API part implementing the java.awt package for J2SE 5.0</rdfs:comment>
	</owl:Class>
	<owl:Class rdf:about="&j2se-5_0;JavaAwtEvent">
		<rdfs:subClassOf rdf:resource="&j2se-1_4;JavaAwtEvent"/>
		<rdfs:seeAlso rdf:resource="&j2se-5_0;JavaAwt"/>
		<rdfs:seeAlso rdf:resource="&j2se-5_0;JavaUtil"/>
		<rdfs:seeAlso rdf:resource="&j2se-5_0;JavaAwtFont"/>
		<rdfs:seeAlso rdf:resource="&j2se-5_0;JavaText"/>
		<rdfs:seeAlso rdf:resource="&j2se-5_0;JavaLang"/>
		<rdfs:comment xml:lang="en">Java API part implementing the java.awt.event package for J2SE 5.0</rdfs:comment>
	</owl:Class>
	<owl:Class rdf:about="&j2se-5_0;JavaAwtImage">
		<rdfs:subClassOf rdf:resource="&j2se-1_4;JavaAwtImage"/>
		<rdfs:seeAlso rdf:resource="&j2se-5_0;JavaAwt"/>
		<rdfs:seeAlso rdf:resource="&j2se-5_0;JavaMath"/>
		<rdfs:seeAlso rdf:resource="&j2se-5_0;JavaUtil"/>
		<rdfs:seeAlso rdf:resource="&j2se-5_0;JavaLang"/>
		<rdfs:seeAlso rdf:resource="&j2se-5_0;JavaAwtColor"/>
		<rdfs:seeAlso rdf:resource="&j2se-5_0;JavaAwtGeom"/>
		<rdfs:comment xml:lang="en">Java API part implementing the java.awt.image package for J2SE 5.0</rdfs:comment>
	</owl:Class>
	<owl:Class rdf:about="&j2se-5_0;JavaAwtImageRenderable">
		<owl:equivalentClass rdf:resource="&j2se-1_4;JavaAwtImageRenderable"/>
		<rdfs:subClassOf rdf:resource="&java;JavaAPIPart"/>
		<rdfs:seeAlso rdf:resource="&j2se-5_0;JavaAwt"/>
		<rdfs:seeAlso rdf:resource="&j2se-5_0;JavaUtil"/>
		<rdfs:seeAlso rdf:resource="&j2se-5_0;JavaIo"/>
		<rdfs:seeAlso rdf:resource="&j2se-5_0;JavaLang"/>
		<rdfs:seeAlso rdf:resource="&j2se-5_0;JavaAwtImage"/>
		<rdfs:seeAlso rdf:resource="&j2se-5_0;JavaAwtGeom"/>
		<rdfs:comment xml:lang="en">Java API part implementing the java.awt.image.renderable package for J2SE 5.0</rdfs:comment>
	</owl:Class>
	<owl:Class rdf:about="&j2se-5_0;JavaAwtGeom">
		<owl:equivalentClass rdf:resource="&j2se-1_4;JavaAwtGeom"/>
		<rdfs:subClassOf rdf:resource="&java;JavaAPIPart"/>
		<rdfs:seeAlso rdf:resource="&j2se-5_0;JavaAwt"/>
		<rdfs:seeAlso rdf:resource="&j2se-5_0;JavaLang"/>
		<rdfs:seeAlso rdf:resource="&j2se-5_0;JavaIo"/>
		<rdfs:comment xml:lang="en">Java API part implementing the java.awt.geom package for J2SE 5.0</rdfs:comment>
	</owl:Class>
	<owl:Class rdf:about="&j2se-5_0;JavaAwtIm">
		<owl:equivalentClass rdf:resource="&j2se-1_4;JavaAwtIm"/>
		<rdfs:subClassOf rdf:resource="&java;JavaAPIPart"/>
		<rdfs:seeAlso rdf:resource="&j2se-5_0;JavaAwt"/>
		<rdfs:seeAlso rdf:resource="&j2se-5_0;JavaText"/>
		<rdfs:seeAlso rdf:resource="&j2se-5_0;JavaLang"/>
		<rdfs:seeAlso rdf:resource="&j2se-5_0;JavaUtil"/>
		<rdfs:seeAlso rdf:resource="&j2se-5_0;JavaAwtFont"/>
		<rdfs:comment xml:lang="en">Java API part implementing the java.awt.im package for J2SE 5.0</rdfs:comment>
	</owl:Class>
	<owl:Class rdf:about="&j2se-5_0;JavaAwtImSpi">
		<owl:equivalentClass rdf:resource="&j2se-1_4;JavaAwtImSpi"/>
		<rdfs:subClassOf rdf:resource="&java;JavaAPIPart"/>
		<rdfs:seeAlso rdf:resource="&j2se-5_0;JavaAwt"/>
		<rdfs:seeAlso rdf:resource="&j2se-5_0;JavaText"/>
		<rdfs:seeAlso rdf:resource="&j2se-5_0;JavaLang"/>
		<rdfs:seeAlso rdf:resource="&j2se-5_0;JavaUtil"/>
		<rdfs:seeAlso rdf:resource="&j2se-5_0;JavaxSwing"/>
		<rdfs:seeAlso rdf:resource="&j2se-5_0;JavaAwtFont"/>
		<rdfs:seeAlso rdf:resource="&j2se-5_0;JavaAwtIm"/>
		<rdfs:comment xml:lang="en">Java API part implementing the java.awt.im.spi package for J2SE 5.0</rdfs:comment>
	</owl:Class>
	<owl:Class rdf:about="&j2se-5_0;JavaAwtColor">
		<rdfs:subClassOf rdf:resource="&j2se-1_4;JavaAwtColor"/>
		<rdfs:seeAlso rdf:resource="&j2se-5_0;JavaLang"/>
		<rdfs:seeAlso rdf:resource="&j2se-5_0;JavaIo"/>
		<rdfs:comment xml:lang="en">Java API part implementing the java.awt.color package for J2SE 5.0</rdfs:comment>
	</owl:Class>
	<owl:Class rdf:about="&j2se-5_0;JavaAwtDatatransfer">
		<rdfs:subClassOf rdf:resource="&j2se-1_4;JavaAwtDatatransfer"/>
		<rdfs:seeAlso rdf:resource="&j2se-5_0;JavaUtil"/>
		<rdfs:seeAlso rdf:resource="&j2se-5_0;JavaIo"/>
		<rdfs:seeAlso rdf:resource="&j2se-5_0;JavaLang"/>
		<rdfs:comment xml:lang="en">Java API part implementing the java.awt.datatransfer package for J2SE 5.0</rdfs:comment>
	</owl:Class>
	<owl:Class rdf:about="&j2se-5_0;JavaAwtDnd">
		<rdfs:subClassOf rdf:resource="&j2se-1_4;JavaAwtDnd"/>
		<rdfs:seeAlso rdf:resource="&j2se-5_0;JavaAwtDatatransfer"/>
		<rdfs:seeAlso rdf:resource="&j2se-5_0;JavaIo"/>
		<rdfs:seeAlso rdf:resource="&j2se-5_0;JavaAwt"/>
		<rdfs:seeAlso rdf:resource="&j2se-5_0;JavaUtil"/>
		<rdfs:seeAlso rdf:resource="&j2se-5_0;JavaAwtEvent"/>
		<rdfs:seeAlso rdf:resource="&j2se-5_0;JavaLang"/>
		<rdfs:comment xml:lang="en">Java API part implementing the java.awt.dnd package for J2SE 5.0</rdfs:comment>
	</owl:Class>
	<owl:Class rdf:about="&j2se-5_0;JavaAwtFont">
		<owl:equivalentClass rdf:resource="&j2se-1_4;JavaAwtFont"/>
		<rdfs:subClassOf rdf:resource="&java;JavaAPIPart"/>
		<rdfs:seeAlso rdf:resource="&j2se-5_0;JavaAwt"/>
		<rdfs:seeAlso rdf:resource="&j2se-5_0;JavaUtil"/>
		<rdfs:seeAlso rdf:resource="&j2se-5_0;JavaIo"/>
		<rdfs:seeAlso rdf:resource="&j2se-5_0;JavaText"/>
		<rdfs:seeAlso rdf:resource="&j2se-5_0;JavaLang"/>
		<rdfs:seeAlso rdf:resource="&j2se-5_0;JavaAwtGeom"/>
		<rdfs:comment xml:lang="en">Java API part implementing the java.awt.font package for J2SE 5.0</rdfs:comment>
	</owl:Class>
	<owl:Class rdf:about="&j2se-5_0;JavaAwtPrint">
		<owl:equivalentClass rdf:resource="&j2se-1_4;JavaAwtPrint"/>
		<rdfs:subClassOf rdf:resource="&java;JavaAPIPart"/>
		<rdfs:seeAlso rdf:resource="&j2se-5_0;JavaAwt"/>
		<rdfs:seeAlso rdf:resource="&j2se-5_0;JavaxPrint"/>
		<rdfs:seeAlso rdf:resource="&j2se-5_0;JavaxPrintAttribute"/>
		<rdfs:seeAlso rdf:resource="&j2se-5_0;JavaLang"/>
		<rdfs:seeAlso rdf:resource="&j2se-5_0;JavaIo"/>
		<rdfs:comment xml:lang="en">Java API part implementing the java.awt.print package for J2SE 5.0</rdfs:comment>
	</owl:Class>
	<owl:Class rdf:about="&j2se-5_0;JavaText">
		<rdfs:subClassOf rdf:resource="&j2se-1_4;JavaText"/>
		<rdfs:seeAlso rdf:resource="&j2se-5_0;JavaUtil"/>
		<rdfs:seeAlso rdf:resource="&j2se-5_0;JavaIo"/>
		<rdfs:seeAlso rdf:resource="&j2se-5_0;JavaLang"/>
		<rdfs:comment xml:lang="en">Java API part implementing the java.text package for J2SE 5.0</rdfs:comment>
	</owl:Class>
	<owl:Class rdf:about="&j2se-5_0;JavaBeans">
		<rdfs:subClassOf rdf:resource="&j2se-1_4;JavaBeans"/>
		<rdfs:seeAlso rdf:resource="&j2se-5_0;JavaAwt"/>
		<rdfs:seeAlso rdf:resource="&j2se-5_0;JavaLangReflect"/>
		<rdfs:seeAlso rdf:resource="&j2se-5_0;JavaUtil"/>
		<rdfs:seeAlso rdf:resource="&j2se-5_0;JavaIo"/>
		<rdfs:seeAlso rdf:resource="&j2se-5_0;JavaApplet"/>
		<rdfs:seeAlso rdf:resource="&j2se-5_0;JavaBeansBeancontext"/>
		<rdfs:seeAlso rdf:resource="&j2se-5_0;JavaLang"/>
		<rdfs:comment xml:lang="en">Java API part implementing the java.beans package for J2SE 5.0</rdfs:comment>
	</owl:Class>
	<owl:Class rdf:about="&j2se-5_0;JavaBeansBeancontext">
		<owl:equivalentClass rdf:resource="&j2se-1_4;JavaBeansBeancontext"/>
		<rdfs:subClassOf rdf:resource="&java;JavaAPIPart"/>
		<rdfs:seeAlso rdf:resource="&j2se-5_0;JavaNet"/>
		<rdfs:seeAlso rdf:resource="&j2se-5_0;JavaIo"/>
		<rdfs:seeAlso rdf:resource="&j2se-5_0;JavaAwt"/>
		<rdfs:seeAlso rdf:resource="&j2se-5_0;JavaUtil"/>
		<rdfs:seeAlso rdf:resource="&j2se-5_0;JavaLang"/>
		<rdfs:seeAlso rdf:resource="&j2se-5_0;JavaBeans"/>
		<rdfs:comment xml:lang="en">Java API part implementing the java.beans.beancontext package for J2SE 5.0</rdfs:comment>
	</owl:Class>
	<owl:Class rdf:about="&j2se-5_0;JavaRmi">
		<owl:equivalentClass rdf:resource="&j2se-1_4;JavaRmi"/>
		<rdfs:subClassOf rdf:resource="&java;JavaAPIPart"/>
		<rdfs:seeAlso rdf:resource="&j2se-5_0;JavaLang"/>
		<rdfs:seeAlso rdf:resource="&j2se-5_0;JavaIo"/>
		<rdfs:comment xml:lang="en">Java API part implementing the java.rmi package for J2SE 5.0</rdfs:comment>
	</owl:Class>
	<owl:Class rdf:about="&j2se-5_0;JavaRmiActivation">
		<owl:equivalentClass rdf:resource="&j2se-1_4;JavaRmiActivation"/>
		<rdfs:subClassOf rdf:resource="&java;JavaAPIPart"/>
		<rdfs:seeAlso rdf:resource="&j2se-5_0;JavaRmi"/>
		<rdfs:seeAlso rdf:resource="&j2se-5_0;JavaUtil"/>
		<rdfs:seeAlso rdf:resource="&j2se-5_0;JavaIo"/>
		<rdfs:seeAlso rdf:resource="&j2se-5_0;JavaRmiServer"/>
		<rdfs:seeAlso rdf:resource="&j2se-5_0;JavaLang"/>
		<rdfs:comment xml:lang="en">Java API part implementing the java.rmi.activation package for J2SE 5.0</rdfs:comment>
	</owl:Class>
	<owl:Class rdf:about="&j2se-5_0;JavaRmiServer">
		<rdfs:subClassOf rdf:resource="&j2se-1_4;JavaRmiServer"/>
		<rdfs:seeAlso rdf:resource="&j2se-5_0;JavaLangReflect"/>
		<rdfs:seeAlso rdf:resource="&j2se-5_0;JavaRmi"/>
		<rdfs:seeAlso rdf:resource="&j2se-5_0;JavaNet"/>
		<rdfs:seeAlso rdf:resource="&j2se-5_0;JavaIo"/>
		<rdfs:seeAlso rdf:resource="&j2se-5_0;JavaLang"/>
		<rdfs:comment xml:lang="en">Java API part implementing the java.rmi.server package for J2SE 5.0</rdfs:comment>
	</owl:Class>
	<owl:Class rdf:about="&j2se-5_0;JavaRmiDgc">
		<owl:equivalentClass rdf:resource="&j2se-1_4;JavaRmiDgc"/>
		<rdfs:subClassOf rdf:resource="&java;JavaAPIPart"/>
		<rdfs:seeAlso rdf:resource="&j2se-5_0;JavaLang"/>
		<rdfs:seeAlso rdf:resource="&j2se-5_0;JavaRmi"/>
		<rdfs:seeAlso rdf:resource="&j2se-5_0;JavaIo"/>
		<rdfs:comment xml:lang="en">Java API part implementing the java.rmi.dgc package for J2SE 5.0</rdfs:comment>
	</owl:Class>
	<owl:Class rdf:about="&j2se-5_0;JavaRmiRegistry">
		<owl:equivalentClass rdf:resource="&j2se-1_4;JavaRmiRegistry"/>
		<rdfs:subClassOf rdf:resource="&java;JavaAPIPart"/>
		<rdfs:seeAlso rdf:resource="&j2se-5_0;JavaRmiServer"/>
		<rdfs:seeAlso rdf:resource="&j2se-5_0;JavaLang"/>
		<rdfs:seeAlso rdf:resource="&j2se-5_0;JavaRmi"/>
		<rdfs:comment xml:lang="en">Java API part implementing the java.rmi.registry package for J2SE 5.0</rdfs:comment>
	</owl:Class>
	<owl:Class rdf:about="&j2se-5_0;JavaSql">
		<owl:equivalentClass rdf:resource="&j2se-1_4;JavaSql"/>
		<rdfs:subClassOf rdf:resource="&java;JavaAPIPart"/>
		<rdfs:seeAlso rdf:resource="&j2se-5_0;JavaMath"/>
		<rdfs:seeAlso rdf:resource="&j2se-5_0;JavaSecurity"/>
		<rdfs:seeAlso rdf:resource="&j2se-5_0;JavaNet"/>
		<rdfs:seeAlso rdf:resource="&j2se-5_0;JavaUtil"/>
		<rdfs:seeAlso rdf:resource="&j2se-5_0;JavaIo"/>
		<rdfs:seeAlso rdf:resource="&j2se-5_0;JavaLang"/>
		<rdfs:comment xml:lang="en">Java API part implementing the java.sql package for J2SE 5.0</rdfs:comment>
	</owl:Class>
	<owl:Class rdf:about="&j2se-5_0;OrgW3cDom">
		<rdfs:subClassOf rdf:resource="&j2se-1_4;OrgW3cDom"/>
		<rdfs:seeAlso rdf:resource="&j2se-5_0;JavaLang"/>
		<rdfs:comment xml:lang="en">Java API part implementing the org.w3c.dom package for J2SE 5.0</rdfs:comment>
	</owl:Class>
	<owl:Class rdf:about="&j2se-5_0;OrgW3cDomLs">
		<rdfs:subClassOf rdf:resource="&java;JavaAPIPart"/>
		<rdfs:seeAlso rdf:resource="&j2se-5_0;OrgW3cDom"/>
		<rdfs:seeAlso rdf:resource="&j2se-5_0;OrgW3cDomEvents"/>
		<rdfs:seeAlso rdf:resource="&j2se-5_0;OrgW3cDomTraversal"/>
		<rdfs:seeAlso rdf:resource="&j2se-5_0;JavaIo"/>
		<rdfs:seeAlso rdf:resource="&j2se-5_0;JavaLang"/>
		<rdfs:comment xml:lang="en">Java API part implementing the org.w3c.dom.ls package for J2SE 5.0</rdfs:comment>
	</owl:Class>
	<owl:Class rdf:about="&j2se-5_0;OrgW3cDomBootstrap">
		<rdfs:subClassOf rdf:resource="&java;JavaAPIPart"/>
		<rdfs:seeAlso rdf:resource="&j2se-5_0;OrgW3cDom"/>
		<rdfs:seeAlso rdf:resource="&j2se-5_0;JavaLang"/>
		<rdfs:comment xml:lang="en">Java API part implementing the org.w3c.dom.bootstrap package for J2SE 5.0</rdfs:comment>
	</owl:Class>
	<owl:Class rdf:about="&j2se-5_0;OrgW3cDomCss">
		<rdfs:subClassOf rdf:resource="&j2se-1_4;OrgW3cDomCss"/>
		<rdfs:seeAlso rdf:resource="&j2se-5_0;OrgW3cDom"/>
		<rdfs:seeAlso rdf:resource="&j2se-5_0;JavaLang"/>
		<rdfs:seeAlso rdf:resource="&j2se-5_0;OrgW3cDomViews"/>
		<rdfs:seeAlso rdf:resource="&j2se-5_0;OrgW3cDomStylesheets"/>
		<rdfs:comment xml:lang="en">Java API part implementing the org.w3c.dom.css package for J2SE 5.0</rdfs:comment>
	</owl:Class>
	<owl:Class rdf:about="&j2se-5_0;OrgW3cDomStylesheets">
		<owl:equivalentClass rdf:resource="&j2se-1_4;OrgW3cDomStylesheets"/>
		<rdfs:subClassOf rdf:resource="&java;JavaAPIPart"/>
		<rdfs:seeAlso rdf:resource="&j2se-5_0;OrgW3cDom"/>
		<rdfs:seeAlso rdf:resource="&j2se-5_0;JavaLang"/>
		<rdfs:comment xml:lang="en">Java API part implementing the org.w3c.dom.stylesheets package for J2SE 5.0</rdfs:comment>
	</owl:Class>
	<owl:Class rdf:about="&j2se-5_0;OrgW3cDomViews">
		<owl:equivalentClass rdf:resource="&j2se-1_4;OrgW3cDomViews"/>
		<rdfs:subClassOf rdf:resource="&java;JavaAPIPart"/>
		<rdfs:comment xml:lang="en">Java API part implementing the org.w3c.dom.views package for J2SE 5.0</rdfs:comment>
	</owl:Class>
	<owl:Class rdf:about="&j2se-5_0;OrgW3cDomEvents">
		<owl:equivalentClass rdf:resource="&j2se-1_4;OrgW3cDomEvents"/>
		<rdfs:subClassOf rdf:resource="&java;JavaAPIPart"/>
		<rdfs:seeAlso rdf:resource="&j2se-5_0;OrgW3cDom"/>
		<rdfs:seeAlso rdf:resource="&j2se-5_0;JavaLang"/>
		<rdfs:seeAlso rdf:resource="&j2se-5_0;OrgW3cDomViews"/>
		<rdfs:comment xml:lang="en">Java API part implementing the org.w3c.dom.events package for J2SE 5.0</rdfs:comment>
	</owl:Class>
	<owl:Class rdf:about="&j2se-5_0;OrgW3cDomHtml">
		<rdfs:subClassOf rdf:resource="&j2se-1_4;OrgW3cDomHtml"/>
		<rdfs:seeAlso rdf:resource="&j2se-5_0;OrgW3cDom"/>
		<rdfs:seeAlso rdf:resource="&j2se-5_0;JavaLang"/>
		<rdfs:comment xml:lang="en">Java API part implementing the org.w3c.dom.html package for J2SE 5.0</rdfs:comment>
	</owl:Class>
	<owl:Class rdf:about="&j2se-5_0;OrgW3cDomTraversal">
		<owl:equivalentClass rdf:resource="&j2se-1_4;OrgW3cDomTraversal"/>
		<rdfs:subClassOf rdf:resource="&java;JavaAPIPart"/>
		<rdfs:seeAlso rdf:resource="&j2se-5_0;OrgW3cDom"/>
		<rdfs:comment xml:lang="en">Java API part implementing the org.w3c.dom.traversal package for J2SE 5.0</rdfs:comment>
	</owl:Class>
	<owl:Class rdf:about="&j2se-5_0;OrgW3cDomRanges">
		<rdfs:subClassOf rdf:resource="&java;JavaAPIPart"/>
		<rdfs:seeAlso rdf:resource="&j2se-5_0;OrgW3cDom"/>
		<rdfs:seeAlso rdf:resource="&j2se-5_0;JavaLang"/>
		<rdfs:comment xml:lang="en">Java API part implementing the org.w3c.dom.ranges package for J2SE 5.0</rdfs:comment>
	</owl:Class>
	<owl:Class rdf:about="&j2se-5_0;OrgOmgCORBA_2_3">
		<owl:equivalentClass rdf:resource="&j2se-1_4;OrgOmgCORBA_2_3"/>
		<rdfs:subClassOf rdf:resource="&java;JavaAPIPart"/>
		<rdfs:seeAlso rdf:resource="&j2se-5_0;OrgOmgCORBA"/>
		<rdfs:seeAlso rdf:resource="&j2se-5_0;OrgOmgCORBAPortable"/>
		<rdfs:seeAlso rdf:resource="&j2se-5_0;JavaLang"/>
		<rdfs:comment xml:lang="en">Java API part implementing the org.omg.CORBA_2_3 package for J2SE 5.0</rdfs:comment>
	</owl:Class>
	<owl:Class rdf:about="&j2se-5_0;OrgOmgCORBA_2_3Portable">
		<owl:equivalentClass rdf:resource="&j2se-1_4;OrgOmgCORBA_2_3Portable"/>
		<rdfs:subClassOf rdf:resource="&java;JavaAPIPart"/>
		<rdfs:seeAlso rdf:resource="&j2se-5_0;OrgOmgCORBA"/>
		<rdfs:seeAlso rdf:resource="&j2se-5_0;OrgOmgCORBAPortable"/>
		<rdfs:seeAlso rdf:resource="&j2se-5_0;JavaLang"/>
		<rdfs:seeAlso rdf:resource="&j2se-5_0;JavaIo"/>
		<rdfs:comment xml:lang="en">Java API part implementing the org.omg.CORBA_2_3.portable package for J2SE 5.0</rdfs:comment>
	</owl:Class>
	<owl:Class rdf:about="&j2se-5_0;OrgOmgCORBA">
		<rdfs:subClassOf rdf:resource="&j2se-1_4;OrgOmgCORBA"/>
		<rdfs:seeAlso rdf:resource="&j2se-5_0;JavaMath"/>
		<rdfs:seeAlso rdf:resource="&j2se-5_0;JavaUtil"/>
		<rdfs:seeAlso rdf:resource="&j2se-5_0;JavaIo"/>
		<rdfs:seeAlso rdf:resource="&j2se-5_0;JavaApplet"/>
		<rdfs:seeAlso rdf:resource="&j2se-5_0;OrgOmgCORBAPortable"/>
		<rdfs:seeAlso rdf:resource="&j2se-5_0;JavaLang"/>
		<rdfs:comment xml:lang="en">Java API part implementing the org.omg.CORBA package for J2SE 5.0</rdfs:comment>
	</owl:Class>
	<owl:Class rdf:about="&j2se-5_0;OrgOmgCORBAPortable">
		<rdfs:subClassOf rdf:resource="&j2se-1_4;OrgOmgCORBAPortable"/>
		<rdfs:seeAlso rdf:resource="&j2se-5_0;OrgOmgCORBA"/>
		<rdfs:seeAlso rdf:resource="&j2se-5_0;JavaMath"/>
		<rdfs:seeAlso rdf:resource="&j2se-5_0;JavaIo"/>
		<rdfs:seeAlso rdf:resource="&j2se-5_0;OrgOmgCORBA_2_3Portable"/>
		<rdfs:seeAlso rdf:resource="&j2se-5_0;JavaLang"/>
		<rdfs:comment xml:lang="en">Java API part implementing the org.omg.CORBA.portable package for J2SE 5.0</rdfs:comment>
	</owl:Class>
	<owl:Class rdf:about="&j2se-5_0;OrgOmgCORBADynAnyPackage">
		<owl:equivalentClass rdf:resource="&j2se-1_4;OrgOmgCORBADynAnyPackage"/>
		<rdfs:subClassOf rdf:resource="&java;JavaAPIPart"/>
		<rdfs:seeAlso rdf:resource="&j2se-5_0;OrgOmgCORBA"/>
		<rdfs:seeAlso rdf:resource="&j2se-5_0;JavaLang"/>
		<rdfs:comment xml:lang="en">Java API part implementing the org.omg.CORBA.DynAnyPackage package for J2SE 5.0</rdfs:comment>
	</owl:Class>
	<owl:Class rdf:about="&j2se-5_0;OrgOmgCORBAORBPackage">
		<owl:equivalentClass rdf:resource="&j2se-1_4;OrgOmgCORBAORBPackage"/>
		<rdfs:subClassOf rdf:resource="&java;JavaAPIPart"/>
		<rdfs:seeAlso rdf:resource="&j2se-5_0;OrgOmgCORBA"/>
		<rdfs:seeAlso rdf:resource="&j2se-5_0;JavaLang"/>
		<rdfs:comment xml:lang="en">Java API part implementing the org.omg.CORBA.ORBPackage package for J2SE 5.0</rdfs:comment>
	</owl:Class>
	<owl:Class rdf:about="&j2se-5_0;OrgOmgCORBATypeCodePackage">
		<owl:equivalentClass rdf:resource="&j2se-1_4;OrgOmgCORBATypeCodePackage"/>
		<rdfs:subClassOf rdf:resource="&java;JavaAPIPart"/>
		<rdfs:seeAlso rdf:resource="&j2se-5_0;OrgOmgCORBA"/>
		<rdfs:seeAlso rdf:resource="&j2se-5_0;JavaLang"/>
		<rdfs:comment xml:lang="en">Java API part implementing the org.omg.CORBA.TypeCodePackage package for J2SE 5.0</rdfs:comment>
	</owl:Class>
	<owl:Class rdf:about="&j2se-5_0;OrgOmgSendingContext">
		<owl:equivalentClass rdf:resource="&j2se-1_4;OrgOmgSendingContext"/>
		<rdfs:subClassOf rdf:resource="&java;JavaAPIPart"/>
		<rdfs:seeAlso rdf:resource="&j2se-5_0;OrgOmgCORBA"/>
		<rdfs:seeAlso rdf:resource="&j2se-5_0;OrgOmgCORBAPortable"/>
		<rdfs:comment xml:lang="en">Java API part implementing the org.omg.SendingContext package for J2SE 5.0</rdfs:comment>
	</owl:Class>
	<owl:Class rdf:about="&j2se-5_0;OrgOmgCosNaming">
		<rdfs:subClassOf rdf:resource="&j2se-1_4;OrgOmgCosNaming"/>
		<rdfs:seeAlso rdf:resource="&j2se-5_0;OrgOmgCORBA"/>
		<rdfs:seeAlso rdf:resource="&j2se-5_0;OrgOmgPortableServer"/>
		<rdfs:seeAlso rdf:resource="&j2se-5_0;OrgOmgCORBAPortable"/>
		<rdfs:seeAlso rdf:resource="&j2se-5_0;JavaLang"/>
		<rdfs:comment xml:lang="en">Java API part implementing the org.omg.CosNaming package for J2SE 5.0</rdfs:comment>
	</owl:Class>
	<owl:Class rdf:about="&j2se-5_0;OrgOmgCosNamingNamingContextExtPackage">
		<owl:equivalentClass rdf:resource="&j2se-1_4;OrgOmgCosNamingNamingContextExtPackage"/>
		<rdfs:subClassOf rdf:resource="&java;JavaAPIPart"/>
		<rdfs:seeAlso rdf:resource="&j2se-5_0;OrgOmgCORBA"/>
		<rdfs:seeAlso rdf:resource="&j2se-5_0;OrgOmgCORBAPortable"/>
		<rdfs:seeAlso rdf:resource="&j2se-5_0;JavaLang"/>
		<rdfs:comment xml:lang="en">Java API part implementing the org.omg.CosNaming.NamingContextExtPackage package for J2SE 5.0</rdfs:comment>
	</owl:Class>
	<owl:Class rdf:about="&j2se-5_0;OrgOmgCosNamingNamingContextPackage">
		<owl:equivalentClass rdf:resource="&j2se-1_4;OrgOmgCosNamingNamingContextPackage"/>
		<rdfs:subClassOf rdf:resource="&java;JavaAPIPart"/>
		<rdfs:seeAlso rdf:resource="&j2se-5_0;OrgOmgCORBA"/>
		<rdfs:seeAlso rdf:resource="&j2se-5_0;OrgOmgCORBAPortable"/>
		<rdfs:seeAlso rdf:resource="&j2se-5_0;JavaLang"/>
		<rdfs:seeAlso rdf:resource="&j2se-5_0;OrgOmgCosNaming"/>
		<rdfs:comment xml:lang="en">Java API part implementing the org.omg.CosNaming.NamingContextPackage package for J2SE 5.0</rdfs:comment>
	</owl:Class>
	<owl:Class rdf:about="&j2se-5_0;OrgOmgPortableServer">
		<rdfs:subClassOf rdf:resource="&j2se-1_4;OrgOmgPortableServer"/>
		<rdfs:seeAlso rdf:resource="&j2se-5_0;OrgOmgCORBA"/>
		<rdfs:seeAlso rdf:resource="&j2se-5_0;OrgOmgPortableServerPortable"/>
		<rdfs:seeAlso rdf:resource="&j2se-5_0;OrgOmgPortableServerPOAManagerPackage"/>
		<rdfs:seeAlso rdf:resource="&j2se-5_0;OrgOmgPortableServerServantLocatorPackage"/>
		<rdfs:seeAlso rdf:resource="&j2se-5_0;OrgOmgCORBAPortable"/>
		<rdfs:seeAlso rdf:resource="&j2se-5_0;JavaLang"/>
		<rdfs:comment xml:lang="en">Java API part implementing the org.omg.PortableServer package for J2SE 5.0</rdfs:comment>
	</owl:Class>
	<owl:Class rdf:about="&j2se-5_0;OrgOmgPortableServerCurrentPackage">
		<owl:equivalentClass rdf:resource="&j2se-1_4;OrgOmgPortableServerCurrentPackage"/>
		<rdfs:subClassOf rdf:resource="&java;JavaAPIPart"/>
		<rdfs:seeAlso rdf:resource="&j2se-5_0;OrgOmgCORBA"/>
		<rdfs:seeAlso rdf:resource="&j2se-5_0;OrgOmgCORBAPortable"/>
		<rdfs:seeAlso rdf:resource="&j2se-5_0;JavaLang"/>
		<rdfs:comment xml:lang="en">Java API part implementing the org.omg.PortableServer.CurrentPackage package for J2SE 5.0</rdfs:comment>
	</owl:Class>
	<owl:Class rdf:about="&j2se-5_0;OrgOmgPortableServerPOAManagerPackage">
		<owl:equivalentClass rdf:resource="&j2se-1_4;OrgOmgPortableServerPOAManagerPackage"/>
		<rdfs:subClassOf rdf:resource="&java;JavaAPIPart"/>
		<rdfs:seeAlso rdf:resource="&j2se-5_0;OrgOmgCORBA"/>
		<rdfs:seeAlso rdf:resource="&j2se-5_0;OrgOmgCORBAPortable"/>
		<rdfs:seeAlso rdf:resource="&j2se-5_0;JavaLang"/>
		<rdfs:comment xml:lang="en">Java API part implementing the org.omg.PortableServer.POAManagerPackage package for J2SE 5.0</rdfs:comment>
	</owl:Class>
	<owl:Class rdf:about="&j2se-5_0;OrgOmgPortableServerPOAPackage">
		<owl:equivalentClass rdf:resource="&j2se-1_4;OrgOmgPortableServerPOAPackage"/>
		<rdfs:subClassOf rdf:resource="&java;JavaAPIPart"/>
		<rdfs:seeAlso rdf:resource="&j2se-5_0;OrgOmgCORBA"/>
		<rdfs:seeAlso rdf:resource="&j2se-5_0;OrgOmgCORBAPortable"/>
		<rdfs:seeAlso rdf:resource="&j2se-5_0;JavaLang"/>
		<rdfs:comment xml:lang="en">Java API part implementing the org.omg.PortableServer.POAPackage package for J2SE 5.0</rdfs:comment>
	</owl:Class>
	<owl:Class rdf:about="&j2se-5_0;OrgOmgPortableServerPortable">
		<owl:equivalentClass rdf:resource="&j2se-1_4;OrgOmgPortableServerPortable"/>
		<rdfs:subClassOf rdf:resource="&java;JavaAPIPart"/>
		<rdfs:seeAlso rdf:resource="&j2se-5_0;OrgOmgCORBA"/>
		<rdfs:seeAlso rdf:resource="&j2se-5_0;JavaLang"/>
		<rdfs:seeAlso rdf:resource="&j2se-5_0;OrgOmgPortableServer"/>
		<rdfs:comment xml:lang="en">Java API part implementing the org.omg.PortableServer.portable package for J2SE 5.0</rdfs:comment>
	</owl:Class>
	<owl:Class rdf:about="&j2se-5_0;OrgOmgPortableServerServantLocatorPackage">
		<owl:equivalentClass rdf:resource="&j2se-1_4;OrgOmgPortableServerServantLocatorPackage"/>
		<rdfs:subClassOf rdf:resource="&java;JavaAPIPart"/>
		<rdfs:seeAlso rdf:resource="&j2se-5_0;OrgOmgCORBA"/>
		<rdfs:seeAlso rdf:resource="&j2se-5_0;OrgOmgCORBAPortable"/>
		<rdfs:seeAlso rdf:resource="&j2se-5_0;JavaLang"/>
		<rdfs:comment xml:lang="en">Java API part implementing the org.omg.PortableServer.ServantLocatorPackage package for J2SE 5.0</rdfs:comment>
	</owl:Class>
	<owl:Class rdf:about="&j2se-5_0;OrgOmgDynamic">
		<owl:equivalentClass rdf:resource="&j2se-1_4;OrgOmgDynamic"/>
		<rdfs:subClassOf rdf:resource="&java;JavaAPIPart"/>
		<rdfs:seeAlso rdf:resource="&j2se-5_0;OrgOmgCORBA"/>
		<rdfs:seeAlso rdf:resource="&j2se-5_0;OrgOmgCORBAPortable"/>
		<rdfs:seeAlso rdf:resource="&j2se-5_0;JavaLang"/>
		<rdfs:comment xml:lang="en">Java API part implementing the org.omg.Dynamic package for J2SE 5.0</rdfs:comment>
	</owl:Class>
	<owl:Class rdf:about="&j2se-5_0;OrgOmgDynamicAny">
		<rdfs:subClassOf rdf:resource="&j2se-1_4;OrgOmgDynamicAny"/>
		<rdfs:seeAlso rdf:resource="&j2se-5_0;OrgOmgCORBA"/>
		<rdfs:seeAlso rdf:resource="&j2se-5_0;JavaIo"/>
		<rdfs:seeAlso rdf:resource="&j2se-5_0;OrgOmgCORBAPortable"/>
		<rdfs:seeAlso rdf:resource="&j2se-5_0;JavaLang"/>
		<rdfs:comment xml:lang="en">Java API part implementing the org.omg.DynamicAny package for J2SE 5.0</rdfs:comment>
	</owl:Class>
	<owl:Class rdf:about="&j2se-5_0;OrgOmgDynamicAnyDynAnyFactoryPackage">
		<owl:equivalentClass rdf:resource="&j2se-1_4;OrgOmgDynamicAnyDynAnyFactoryPackage"/>
		<rdfs:subClassOf rdf:resource="&java;JavaAPIPart"/>
		<rdfs:seeAlso rdf:resource="&j2se-5_0;OrgOmgCORBA"/>
		<rdfs:seeAlso rdf:resource="&j2se-5_0;OrgOmgCORBAPortable"/>
		<rdfs:seeAlso rdf:resource="&j2se-5_0;JavaLang"/>
		<rdfs:comment xml:lang="en">Java API part implementing the org.omg.DynamicAny.DynAnyFactoryPackage package for J2SE 5.0</rdfs:comment>
	</owl:Class>
	<owl:Class rdf:about="&j2se-5_0;OrgOmgDynamicAnyDynAnyPackage">
		<owl:equivalentClass rdf:resource="&j2se-1_4;OrgOmgDynamicAnyDynAnyPackage"/>
		<rdfs:subClassOf rdf:resource="&java;JavaAPIPart"/>
		<rdfs:seeAlso rdf:resource="&j2se-5_0;OrgOmgCORBA"/>
		<rdfs:seeAlso rdf:resource="&j2se-5_0;OrgOmgCORBAPortable"/>
		<rdfs:seeAlso rdf:resource="&j2se-5_0;JavaLang"/>
		<rdfs:comment xml:lang="en">Java API part implementing the org.omg.DynamicAny.DynAnyPackage package for J2SE 5.0</rdfs:comment>
	</owl:Class>
	<owl:Class rdf:about="&j2se-5_0;OrgOmgIOP">
		<rdfs:subClassOf rdf:resource="&j2se-1_4;OrgOmgIOP"/>
		<rdfs:seeAlso rdf:resource="&j2se-5_0;OrgOmgCORBA"/>
		<rdfs:seeAlso rdf:resource="&j2se-5_0;OrgOmgCORBAPortable"/>
		<rdfs:seeAlso rdf:resource="&j2se-5_0;JavaLang"/>
		<rdfs:comment xml:lang="en">Java API part implementing the org.omg.IOP package for J2SE 5.0</rdfs:comment>
	</owl:Class>
	<owl:Class rdf:about="&j2se-5_0;OrgOmgIOPCodecFactoryPackage">
		<owl:equivalentClass rdf:resource="&j2se-1_4;OrgOmgIOPCodecFactoryPackage"/>
		<rdfs:subClassOf rdf:resource="&java;JavaAPIPart"/>
		<rdfs:seeAlso rdf:resource="&j2se-5_0;OrgOmgCORBA"/>
		<rdfs:seeAlso rdf:resource="&j2se-5_0;OrgOmgCORBAPortable"/>
		<rdfs:seeAlso rdf:resource="&j2se-5_0;JavaLang"/>
		<rdfs:comment xml:lang="en">Java API part implementing the org.omg.IOP.CodecFactoryPackage package for J2SE 5.0</rdfs:comment>
	</owl:Class>
	<owl:Class rdf:about="&j2se-5_0;OrgOmgIOPCodecPackage">
		<owl:equivalentClass rdf:resource="&j2se-1_4;OrgOmgIOPCodecPackage"/>
		<rdfs:subClassOf rdf:resource="&java;JavaAPIPart"/>
		<rdfs:seeAlso rdf:resource="&j2se-5_0;OrgOmgCORBA"/>
		<rdfs:seeAlso rdf:resource="&j2se-5_0;OrgOmgCORBAPortable"/>
		<rdfs:seeAlso rdf:resource="&j2se-5_0;JavaLang"/>
		<rdfs:comment xml:lang="en">Java API part implementing the org.omg.IOP.CodecPackage package for J2SE 5.0</rdfs:comment>
	</owl:Class>
	<owl:Class rdf:about="&j2se-5_0;OrgOmgMessaging">
		<owl:equivalentClass rdf:resource="&j2se-1_4;OrgOmgMessaging"/>
		<rdfs:subClassOf rdf:resource="&java;JavaAPIPart"/>
		<rdfs:seeAlso rdf:resource="&j2se-5_0;OrgOmgCORBA"/>
		<rdfs:seeAlso rdf:resource="&j2se-5_0;OrgOmgCORBAPortable"/>
		<rdfs:seeAlso rdf:resource="&j2se-5_0;JavaLang"/>
		<rdfs:comment xml:lang="en">Java API part implementing the org.omg.Messaging package for J2SE 5.0</rdfs:comment>
	</owl:Class>
	<owl:Class rdf:about="&j2se-5_0;OrgOmgPortableInterceptor">
		<rdfs:subClassOf rdf:resource="&j2se-1_4;OrgOmgPortableInterceptor"/>
		<rdfs:seeAlso rdf:resource="&j2se-5_0;OrgOmgCORBA"/>
		<rdfs:seeAlso rdf:resource="&j2se-5_0;OrgOmgIOP"/>
		<rdfs:seeAlso rdf:resource="&j2se-5_0;OrgOmgCORBAPortable"/>
		<rdfs:seeAlso rdf:resource="&j2se-5_0;JavaLang"/>
		<rdfs:comment xml:lang="en">Java API part implementing the org.omg.PortableInterceptor package for J2SE 5.0</rdfs:comment>
	</owl:Class>
	<owl:Class rdf:about="&j2se-5_0;OrgOmgPortableInterceptorORBInitInfoPackage">
		<owl:equivalentClass rdf:resource="&j2se-1_4;OrgOmgPortableInterceptorORBInitInfoPackage"/>
		<rdfs:subClassOf rdf:resource="&java;JavaAPIPart"/>
		<rdfs:seeAlso rdf:resource="&j2se-5_0;OrgOmgCORBA"/>
		<rdfs:seeAlso rdf:resource="&j2se-5_0;OrgOmgCORBAPortable"/>
		<rdfs:seeAlso rdf:resource="&j2se-5_0;JavaLang"/>
		<rdfs:comment xml:lang="en">Java API part implementing the org.omg.PortableInterceptor.ORBInitInfoPackage package for J2SE 5.0</rdfs:comment>
	</owl:Class>
	<owl:Class rdf:about="&j2se-5_0;OrgOmgStubJavaRmi">
		<owl:equivalentClass rdf:resource="&j2se-1_4;OrgOmgStubJavaRmi"/>
		<rdfs:subClassOf rdf:resource="&java;JavaAPIPart"/>
		<rdfs:seeAlso rdf:resource="&j2se-5_0;JavaxRmiCORBA"/>
		<rdfs:seeAlso rdf:resource="&j2se-5_0;JavaRmi"/>
		<rdfs:comment xml:lang="en">Java API part implementing the org.omg.stub.java.rmi package for J2SE 5.0</rdfs:comment>
	</owl:Class>
	<owl:Class rdf:about="&j2se-5_0;OrgOmgStubJavaxManagementRemoteRmi">
		<rdfs:subClassOf rdf:resource="&java;JavaAPIPart"/>
		<rdfs:seeAlso rdf:resource="&j2se-5_0;OrgOmgCORBA"/>
		<rdfs:seeAlso rdf:resource="&j2se-5_0;JavaxManagementRemote"/>
		<rdfs:seeAlso rdf:resource="&j2se-5_0;JavaRmi"/>
		<rdfs:seeAlso rdf:resource="&j2se-5_0;JavaUtil"/>
		<rdfs:seeAlso rdf:resource="&j2se-5_0;JavaxSecurityAuth"/>
		<rdfs:seeAlso rdf:resource="&j2se-5_0;JavaxRmiCORBA"/>
		<rdfs:seeAlso rdf:resource="&j2se-5_0;OrgOmgCORBAPortable"/>
		<rdfs:seeAlso rdf:resource="&j2se-5_0;OrgOmgCORBA_2_3Portable"/>
		<rdfs:seeAlso rdf:resource="&j2se-5_0;JavaxManagementRemoteRmi"/>
		<rdfs:seeAlso rdf:resource="&j2se-5_0;JavaLang"/>
		<rdfs:seeAlso rdf:resource="&j2se-5_0;JavaxManagement"/>
		<rdfs:comment xml:lang="en">Java API part implementing the org.omg.stub.javax.management.remote.rmi package for J2SE 5.0</rdfs:comment>
	</owl:Class>
	<owl:Class rdf:about="&j2se-5_0;OrgXmlSax">
		<owl:equivalentClass rdf:resource="&j2se-1_4;OrgXmlSax"/>
		<rdfs:subClassOf rdf:resource="&java;JavaAPIPart"/>
		<rdfs:seeAlso rdf:resource="&j2se-5_0;JavaLang"/>
		<rdfs:seeAlso rdf:resource="&j2se-5_0;JavaUtil"/>
		<rdfs:seeAlso rdf:resource="&j2se-5_0;JavaIo"/>
		<rdfs:comment xml:lang="en">Java API part implementing the org.xml.sax package for J2SE 5.0</rdfs:comment>
	</owl:Class>
	<owl:Class rdf:about="&j2se-5_0;OrgXmlSaxExt">
		<rdfs:subClassOf rdf:resource="&j2se-1_4;OrgXmlSaxExt"/>
		<rdfs:seeAlso rdf:resource="&j2se-5_0;OrgXmlSax"/>
		<rdfs:seeAlso rdf:resource="&j2se-5_0;JavaLang"/>
		<rdfs:seeAlso rdf:resource="&j2se-5_0;OrgXmlSaxHelpers"/>
		<rdfs:comment xml:lang="en">Java API part implementing the org.xml.sax.ext package for J2SE 5.0</rdfs:comment>
	</owl:Class>
	<owl:Class rdf:about="&j2se-5_0;OrgXmlSaxHelpers">
		<rdfs:subClassOf rdf:resource="&j2se-1_4;OrgXmlSaxHelpers"/>
		<rdfs:seeAlso rdf:resource="&j2se-5_0;OrgXmlSax"/>
		<rdfs:seeAlso rdf:resource="&j2se-5_0;JavaUtil"/>
		<rdfs:seeAlso rdf:resource="&j2se-5_0;JavaLang"/>
		<rdfs:comment xml:lang="en">Java API part implementing the org.xml.sax.helpers package for J2SE 5.0</rdfs:comment>
	</owl:Class>
	<owl:Class rdf:about="&j2se-5_0;OrgIetfJgss">
		<owl:equivalentClass rdf:resource="&j2se-1_4;OrgIetfJgss"/>
		<rdfs:subClassOf rdf:resource="&java;JavaAPIPart"/>
		<rdfs:seeAlso rdf:resource="&j2se-5_0;JavaSecurity"/>
		<rdfs:seeAlso rdf:resource="&j2se-5_0;JavaLang"/>
		<rdfs:seeAlso rdf:resource="&j2se-5_0;JavaNet"/>
		<rdfs:seeAlso rdf:resource="&j2se-5_0;JavaIo"/>
		<rdfs:comment xml:lang="en">Java API part implementing the org.ietf.jgss package for J2SE 5.0</rdfs:comment>
	</owl:Class>
	<owl:Class rdf:about="&j2se-5_0;JavaxCryptoAPI">
		<rdfs:subClassOf rdf:resource="&j2se-1_4;JavaxCryptoAPI"/>
		<rdfs:comment xml:lang="en">JavaLibrary implementing the javax.crypto package for J2SE 5.0</rdfs:comment>
		<rdfs:comment xml:lang="OWLManchester">platform:comprisesInterfacePart some JavaxCrypto</rdfs:comment>
	</owl:Class>
	<owl:Class rdf:about="&j2se-5_0;JavaxCryptoInterfacesAPI">
		<owl:equivalentClass rdf:resource="&j2se-1_4;JavaxCryptoInterfacesAPI"/>
		<rdfs:subClassOf rdf:resource="&java;JavaAPI"/>
		<rdfs:comment xml:lang="en">JavaLibrary implementing the javax.crypto.interfaces package for J2SE 5.0</rdfs:comment>
		<rdfs:comment xml:lang="OWLManchester">platform:comprisesInterfacePart some JavaxCryptoInterfaces</rdfs:comment>
	</owl:Class>
	<owl:Class rdf:about="&j2se-5_0;JavaxCryptoSpecAPI">
		<rdfs:subClassOf rdf:resource="&j2se-1_4;JavaxCryptoSpecAPI"/>
		<rdfs:comment xml:lang="en">JavaLibrary implementing the javax.crypto.spec package for J2SE 5.0</rdfs:comment>
		<rdfs:comment xml:lang="OWLManchester">platform:comprisesInterfacePart some JavaxCryptoSpec</rdfs:comment>
	</owl:Class>
	<owl:Class rdf:about="&j2se-5_0;JavaxNetAPI">
		<owl:equivalentClass rdf:resource="&j2se-1_4;JavaxNetAPI"/>
		<rdfs:subClassOf rdf:resource="&java;JavaAPI"/>
		<rdfs:comment xml:lang="en">JavaLibrary implementing the javax.net package for J2SE 5.0</rdfs:comment>
		<rdfs:comment xml:lang="OWLManchester">platform:comprisesInterfacePart some JavaxNet</rdfs:comment>
	</owl:Class>
	<owl:Class rdf:about="&j2se-5_0;JavaxNetSslAPI">
		<rdfs:subClassOf rdf:resource="&j2se-1_4;JavaxNetSslAPI"/>
		<rdfs:comment xml:lang="en">JavaLibrary implementing the javax.net.ssl package for J2SE 5.0</rdfs:comment>
		<rdfs:comment xml:lang="OWLManchester">platform:comprisesInterfacePart some JavaxNetSsl</rdfs:comment>
	</owl:Class>
	<owl:Class rdf:about="&j2se-5_0;JavaxSecurityCertAPI">
		<owl:equivalentClass rdf:resource="&j2se-1_4;JavaxSecurityCertAPI"/>
		<rdfs:subClassOf rdf:resource="&java;JavaAPI"/>
		<rdfs:comment xml:lang="en">JavaLibrary implementing the javax.security.cert package for J2SE 5.0</rdfs:comment>
		<rdfs:comment xml:lang="OWLManchester">platform:comprisesInterfacePart some JavaxSecurityCert</rdfs:comment>
	</owl:Class>
	<owl:Class rdf:about="&j2se-5_0;JavaxSecurityAuthAPI">
		<owl:equivalentClass rdf:resource="&j2se-1_4;JavaxSecurityAuthAPI"/>
		<rdfs:subClassOf rdf:resource="&java;JavaAPI"/>
		<rdfs:comment xml:lang="en">JavaLibrary implementing the javax.security.auth package for J2SE 5.0</rdfs:comment>
		<rdfs:comment xml:lang="OWLManchester">platform:comprisesInterfacePart some JavaxSecurityAuth</rdfs:comment>
	</owl:Class>
	<owl:Class rdf:about="&j2se-5_0;JavaxSecurityAuthCallbackAPI">
		<owl:equivalentClass rdf:resource="&j2se-1_4;JavaxSecurityAuthCallbackAPI"/>
		<rdfs:subClassOf rdf:resource="&java;JavaAPI"/>
		<rdfs:comment xml:lang="en">JavaLibrary implementing the javax.security.auth.callback package for J2SE 5.0</rdfs:comment>
		<rdfs:comment xml:lang="OWLManchester">platform:comprisesInterfacePart some JavaxSecurityAuthCallback</rdfs:comment>
	</owl:Class>
	<owl:Class rdf:about="&j2se-5_0;JavaxSecurityAuthX500API">
		<owl:equivalentClass rdf:resource="&j2se-1_4;JavaxSecurityAuthX500API"/>
		<rdfs:subClassOf rdf:resource="&java;JavaAPI"/>
		<rdfs:comment xml:lang="en">JavaLibrary implementing the javax.security.auth.x500 package for J2SE 5.0</rdfs:comment>
		<rdfs:comment xml:lang="OWLManchester">platform:comprisesInterfacePart some JavaxSecurityAuthX500</rdfs:comment>
	</owl:Class>
	<owl:Class rdf:about="&j2se-5_0;JavaxSecurityAuthKerberosAPI">
		<owl:equivalentClass rdf:resource="&j2se-1_4;JavaxSecurityAuthKerberosAPI"/>
		<rdfs:subClassOf rdf:resource="&java;JavaAPI"/>
		<rdfs:comment xml:lang="en">JavaLibrary implementing the javax.security.auth.kerberos package for J2SE 5.0</rdfs:comment>
		<rdfs:comment xml:lang="OWLManchester">platform:comprisesInterfacePart some JavaxSecurityAuthKerberos</rdfs:comment>
	</owl:Class>
	<owl:Class rdf:about="&j2se-5_0;JavaxSecurityAuthLoginAPI">
		<rdfs:subClassOf rdf:resource="&j2se-1_4;JavaxSecurityAuthLoginAPI"/>
		<rdfs:comment xml:lang="en">JavaLibrary implementing the javax.security.auth.login package for J2SE 5.0</rdfs:comment>
		<rdfs:comment xml:lang="OWLManchester">platform:comprisesInterfacePart some JavaxSecurityAuthLogin</rdfs:comment>
	</owl:Class>
	<owl:Class rdf:about="&j2se-5_0;JavaxSecurityAuthSpiAPI">
		<owl:equivalentClass rdf:resource="&j2se-1_4;JavaxSecurityAuthSpiAPI"/>
		<rdfs:subClassOf rdf:resource="&java;JavaAPI"/>
		<rdfs:comment xml:lang="en">JavaLibrary implementing the javax.security.auth.spi package for J2SE 5.0</rdfs:comment>
		<rdfs:comment xml:lang="OWLManchester">platform:comprisesInterfacePart some JavaxSecurityAuthSpi</rdfs:comment>
	</owl:Class>
	<owl:Class rdf:about="&j2se-5_0;JavaxSecuritySaslAPI">
		<rdfs:subClassOf rdf:resource="&java;JavaAPI"/>
		<rdfs:comment xml:lang="en">JavaLibrary implementing the javax.security.sasl package for J2SE 5.0</rdfs:comment>
		<rdfs:comment xml:lang="OWLManchester">platform:comprisesInterfacePart some JavaxSecuritySasl</rdfs:comment>
	</owl:Class>
	<owl:Class rdf:about="&j2se-5_0;JavaxAccessibilityAPI">
		<rdfs:subClassOf rdf:resource="&j2se-1_4;JavaxAccessibilityAPI"/>
		<rdfs:comment xml:lang="en">JavaLibrary implementing the javax.accessibility package for J2SE 5.0</rdfs:comment>
		<rdfs:comment xml:lang="OWLManchester">platform:comprisesInterfacePart some JavaxAccessibility</rdfs:comment>
	</owl:Class>
	<owl:Class rdf:about="&j2se-5_0;JavaxSwingAPI">
		<rdfs:subClassOf rdf:resource="&j2se-1_4;JavaxSwingAPI"/>
		<rdfs:comment xml:lang="en">JavaLibrary implementing the javax.swing package for J2SE 5.0</rdfs:comment>
		<rdfs:comment xml:lang="OWLManchester">platform:comprisesInterfacePart some JavaxSwing</rdfs:comment>
	</owl:Class>
	<owl:Class rdf:about="&j2se-5_0;JavaxSwingTextAPI">
		<rdfs:subClassOf rdf:resource="&j2se-1_4;JavaxSwingTextAPI"/>
		<rdfs:comment xml:lang="en">JavaLibrary implementing the javax.swing.text package for J2SE 5.0</rdfs:comment>
		<rdfs:comment xml:lang="OWLManchester">platform:comprisesInterfacePart some JavaxSwingText</rdfs:comment>
	</owl:Class>
	<owl:Class rdf:about="&j2se-5_0;JavaxSwingTextHtmlAPI">
		<rdfs:subClassOf rdf:resource="&j2se-1_4;JavaxSwingTextHtmlAPI"/>
		<rdfs:comment xml:lang="en">JavaLibrary implementing the javax.swing.text.html package for J2SE 5.0</rdfs:comment>
		<rdfs:comment xml:lang="OWLManchester">platform:comprisesInterfacePart some JavaxSwingTextHtml</rdfs:comment>
	</owl:Class>
	<owl:Class rdf:about="&j2se-5_0;JavaxSwingTextHtmlParserAPI">
		<owl:equivalentClass rdf:resource="&j2se-1_4;JavaxSwingTextHtmlParserAPI"/>
		<rdfs:subClassOf rdf:resource="&java;JavaAPI"/>
		<rdfs:comment xml:lang="en">JavaLibrary implementing the javax.swing.text.html.parser package for J2SE 5.0</rdfs:comment>
		<rdfs:comment xml:lang="OWLManchester">platform:comprisesInterfacePart some JavaxSwingTextHtmlParser</rdfs:comment>
	</owl:Class>
	<owl:Class rdf:about="&j2se-5_0;JavaxSwingTextRtfAPI">
		<owl:equivalentClass rdf:resource="&j2se-1_4;JavaxSwingTextRtfAPI"/>
		<rdfs:subClassOf rdf:resource="&java;JavaAPI"/>
		<rdfs:comment xml:lang="en">JavaLibrary implementing the javax.swing.text.rtf package for J2SE 5.0</rdfs:comment>
		<rdfs:comment xml:lang="OWLManchester">platform:comprisesInterfacePart some JavaxSwingTextRtf</rdfs:comment>
	</owl:Class>
	<owl:Class rdf:about="&j2se-5_0;JavaxSwingEventAPI">
		<rdfs:subClassOf rdf:resource="&j2se-1_4;JavaxSwingEventAPI"/>
		<rdfs:comment xml:lang="en">JavaLibrary implementing the javax.swing.event package for J2SE 5.0</rdfs:comment>
		<rdfs:comment xml:lang="OWLManchester">platform:comprisesInterfacePart some JavaxSwingEvent</rdfs:comment>
	</owl:Class>
	<owl:Class rdf:about="&j2se-5_0;JavaxSwingColorchooserAPI">
		<rdfs:subClassOf rdf:resource="&j2se-1_4;JavaxSwingColorchooserAPI"/>
		<rdfs:comment xml:lang="en">JavaLibrary implementing the javax.swing.colorchooser package for J2SE 5.0</rdfs:comment>
		<rdfs:comment xml:lang="OWLManchester">platform:comprisesInterfacePart some JavaxSwingColorchooser</rdfs:comment>
	</owl:Class>
	<owl:Class rdf:about="&j2se-5_0;JavaxSwingPlafAPI">
		<rdfs:subClassOf rdf:resource="&j2se-1_4;JavaxSwingPlafAPI"/>
		<rdfs:comment xml:lang="en">JavaLibrary implementing the javax.swing.plaf package for J2SE 5.0</rdfs:comment>
		<rdfs:comment xml:lang="OWLManchester">platform:comprisesInterfacePart some JavaxSwingPlaf</rdfs:comment>
	</owl:Class>
	<owl:Class rdf:about="&j2se-5_0;JavaxSwingPlafBasicAPI">
		<rdfs:subClassOf rdf:resource="&j2se-1_4;JavaxSwingPlafBasicAPI"/>
		<rdfs:comment xml:lang="en">JavaLibrary implementing the javax.swing.plaf.basic package for J2SE 5.0</rdfs:comment>
		<rdfs:comment xml:lang="OWLManchester">platform:comprisesInterfacePart some JavaxSwingPlafBasic</rdfs:comment>
	</owl:Class>
	<owl:Class rdf:about="&j2se-5_0;JavaxSwingPlafMetalAPI">
		<rdfs:subClassOf rdf:resource="&j2se-1_4;JavaxSwingPlafMetalAPI"/>
		<rdfs:comment xml:lang="en">JavaLibrary implementing the javax.swing.plaf.metal package for J2SE 5.0</rdfs:comment>
		<rdfs:comment xml:lang="OWLManchester">platform:comprisesInterfacePart some JavaxSwingPlafMetal</rdfs:comment>
	</owl:Class>
	<owl:Class rdf:about="&j2se-5_0;JavaxSwingPlafMultiAPI">
		<rdfs:subClassOf rdf:resource="&j2se-1_4;JavaxSwingPlafMultiAPI"/>
		<rdfs:comment xml:lang="en">JavaLibrary implementing the javax.swing.plaf.multi package for J2SE 5.0</rdfs:comment>
		<rdfs:comment xml:lang="OWLManchester">platform:comprisesInterfacePart some JavaxSwingPlafMulti</rdfs:comment>
	</owl:Class>
	<owl:Class rdf:about="&j2se-5_0;JavaxSwingPlafSynthAPI">
		<rdfs:subClassOf rdf:resource="&java;JavaAPI"/>
		<rdfs:comment xml:lang="en">JavaLibrary implementing the javax.swing.plaf.synth package for J2SE 5.0</rdfs:comment>
		<rdfs:comment xml:lang="OWLManchester">platform:comprisesInterfacePart some JavaxSwingPlafSynth</rdfs:comment>
	</owl:Class>
	<owl:Class rdf:about="&j2se-5_0;JavaxSwingTreeAPI">
		<rdfs:subClassOf rdf:resource="&j2se-1_4;JavaxSwingTreeAPI"/>
		<rdfs:comment xml:lang="en">JavaLibrary implementing the javax.swing.tree package for J2SE 5.0</rdfs:comment>
		<rdfs:comment xml:lang="OWLManchester">platform:comprisesInterfacePart some JavaxSwingTree</rdfs:comment>
	</owl:Class>
	<owl:Class rdf:about="&j2se-5_0;JavaxSwingBorderAPI">
		<owl:equivalentClass rdf:resource="&j2se-1_4;JavaxSwingBorderAPI"/>
		<rdfs:subClassOf rdf:resource="&java;JavaAPI"/>
		<rdfs:comment xml:lang="en">JavaLibrary implementing the javax.swing.border package for J2SE 5.0</rdfs:comment>
		<rdfs:comment xml:lang="OWLManchester">platform:comprisesInterfacePart some JavaxSwingBorder</rdfs:comment>
	</owl:Class>
	<owl:Class rdf:about="&j2se-5_0;JavaxSwingFilechooserAPI">
		<owl:equivalentClass rdf:resource="&j2se-1_4;JavaxSwingFilechooserAPI"/>
		<rdfs:subClassOf rdf:resource="&java;JavaAPI"/>
		<rdfs:comment xml:lang="en">JavaLibrary implementing the javax.swing.filechooser package for J2SE 5.0</rdfs:comment>
		<rdfs:comment xml:lang="OWLManchester">platform:comprisesInterfacePart some JavaxSwingFilechooser</rdfs:comment>
	</owl:Class>
	<owl:Class rdf:about="&j2se-5_0;JavaxSwingTableAPI">
		<rdfs:subClassOf rdf:resource="&j2se-1_4;JavaxSwingTableAPI"/>
		<rdfs:comment xml:lang="en">JavaLibrary implementing the javax.swing.table package for J2SE 5.0</rdfs:comment>
		<rdfs:comment xml:lang="OWLManchester">platform:comprisesInterfacePart some JavaxSwingTable</rdfs:comment>
	</owl:Class>
	<owl:Class rdf:about="&j2se-5_0;JavaxSwingUndoAPI">
		<owl:equivalentClass rdf:resource="&j2se-1_4;JavaxSwingUndoAPI"/>
		<rdfs:subClassOf rdf:resource="&java;JavaAPI"/>
		<rdfs:comment xml:lang="en">JavaLibrary implementing the javax.swing.undo package for J2SE 5.0</rdfs:comment>
		<rdfs:comment xml:lang="OWLManchester">platform:comprisesInterfacePart some JavaxSwingUndo</rdfs:comment>
	</owl:Class>
	<owl:Class rdf:about="&j2se-5_0;JavaxManagementAPI">
		<rdfs:subClassOf rdf:resource="&java;JavaAPI"/>
		<rdfs:comment xml:lang="en">JavaLibrary implementing the javax.management package for J2SE 5.0</rdfs:comment>
		<rdfs:comment xml:lang="OWLManchester">platform:comprisesInterfacePart some JavaxManagement</rdfs:comment>
	</owl:Class>
	<owl:Class rdf:about="&j2se-5_0;JavaxManagementOpenmbeanAPI">
		<rdfs:subClassOf rdf:resource="&java;JavaAPI"/>
		<rdfs:comment xml:lang="en">JavaLibrary implementing the javax.management.openmbean package for J2SE 5.0</rdfs:comment>
		<rdfs:comment xml:lang="OWLManchester">platform:comprisesInterfacePart some JavaxManagementOpenmbean</rdfs:comment>
	</owl:Class>
	<owl:Class rdf:about="&j2se-5_0;JavaxManagementLoadingAPI">
		<rdfs:subClassOf rdf:resource="&java;JavaAPI"/>
		<rdfs:comment xml:lang="en">JavaLibrary implementing the javax.management.loading package for J2SE 5.0</rdfs:comment>
		<rdfs:comment xml:lang="OWLManchester">platform:comprisesInterfacePart some JavaxManagementLoading</rdfs:comment>
	</owl:Class>
	<owl:Class rdf:about="&j2se-5_0;JavaxManagementModelmbeanAPI">
		<rdfs:subClassOf rdf:resource="&java;JavaAPI"/>
		<rdfs:comment xml:lang="en">JavaLibrary implementing the javax.management.modelmbean package for J2SE 5.0</rdfs:comment>
		<rdfs:comment xml:lang="OWLManchester">platform:comprisesInterfacePart some JavaxManagementModelmbean</rdfs:comment>
	</owl:Class>
	<owl:Class rdf:about="&j2se-5_0;JavaxManagementMonitorAPI">
		<rdfs:subClassOf rdf:resource="&java;JavaAPI"/>
		<rdfs:comment xml:lang="en">JavaLibrary implementing the javax.management.monitor package for J2SE 5.0</rdfs:comment>
		<rdfs:comment xml:lang="OWLManchester">platform:comprisesInterfacePart some JavaxManagementMonitor</rdfs:comment>
	</owl:Class>
	<owl:Class rdf:about="&j2se-5_0;JavaxManagementRelationAPI">
		<rdfs:subClassOf rdf:resource="&java;JavaAPI"/>
		<rdfs:comment xml:lang="en">JavaLibrary implementing the javax.management.relation package for J2SE 5.0</rdfs:comment>
		<rdfs:comment xml:lang="OWLManchester">platform:comprisesInterfacePart some JavaxManagementRelation</rdfs:comment>
	</owl:Class>
	<owl:Class rdf:about="&j2se-5_0;JavaxManagementRemoteAPI">
		<rdfs:subClassOf rdf:resource="&java;JavaAPI"/>
		<rdfs:comment xml:lang="en">JavaLibrary implementing the javax.management.remote package for J2SE 5.0</rdfs:comment>
		<rdfs:comment xml:lang="OWLManchester">platform:comprisesInterfacePart some JavaxManagementRemote</rdfs:comment>
	</owl:Class>
	<owl:Class rdf:about="&j2se-5_0;JavaxManagementRemoteRmiAPI">
		<rdfs:subClassOf rdf:resource="&java;JavaAPI"/>
		<rdfs:comment xml:lang="en">JavaLibrary implementing the javax.management.remote.rmi package for J2SE 5.0</rdfs:comment>
		<rdfs:comment xml:lang="OWLManchester">platform:comprisesInterfacePart some JavaxManagementRemoteRmi</rdfs:comment>
	</owl:Class>
	<owl:Class rdf:about="&j2se-5_0;JavaxManagementTimerAPI">
		<rdfs:subClassOf rdf:resource="&java;JavaAPI"/>
		<rdfs:comment xml:lang="en">JavaLibrary implementing the javax.management.timer package for J2SE 5.0</rdfs:comment>
		<rdfs:comment xml:lang="OWLManchester">platform:comprisesInterfacePart some JavaxManagementTimer</rdfs:comment>
	</owl:Class>
	<owl:Class rdf:about="&j2se-5_0;JavaxActivityAPI">
		<rdfs:subClassOf rdf:resource="&java;JavaAPI"/>
		<rdfs:comment xml:lang="en">JavaLibrary implementing the javax.activity package for J2SE 5.0</rdfs:comment>
		<rdfs:comment xml:lang="OWLManchester">platform:comprisesInterfacePart some JavaxActivity</rdfs:comment>
	</owl:Class>
	<owl:Class rdf:about="&j2se-5_0;JavaxImageioAPI">
		<owl:equivalentClass rdf:resource="&j2se-1_4;JavaxImageioAPI"/>
		<rdfs:subClassOf rdf:resource="&java;JavaAPI"/>
		<rdfs:comment xml:lang="en">JavaLibrary implementing the javax.imageio package for J2SE 5.0</rdfs:comment>
		<rdfs:comment xml:lang="OWLManchester">platform:comprisesInterfacePart some JavaxImageio</rdfs:comment>
	</owl:Class>
	<owl:Class rdf:about="&j2se-5_0;JavaxImageioMetadataAPI">
		<rdfs:subClassOf rdf:resource="&j2se-1_4;JavaxImageioMetadataAPI"/>
		<rdfs:comment xml:lang="en">JavaLibrary implementing the javax.imageio.metadata package for J2SE 5.0</rdfs:comment>
		<rdfs:comment xml:lang="OWLManchester">platform:comprisesInterfacePart some JavaxImageioMetadata</rdfs:comment>
	</owl:Class>
	<owl:Class rdf:about="&j2se-5_0;JavaxImageioEventAPI">
		<owl:equivalentClass rdf:resource="&j2se-1_4;JavaxImageioEventAPI"/>
		<rdfs:subClassOf rdf:resource="&java;JavaAPI"/>
		<rdfs:comment xml:lang="en">JavaLibrary implementing the javax.imageio.event package for J2SE 5.0</rdfs:comment>
		<rdfs:comment xml:lang="OWLManchester">platform:comprisesInterfacePart some JavaxImageioEvent</rdfs:comment>
	</owl:Class>
	<owl:Class rdf:about="&j2se-5_0;JavaxImageioPluginsBmpAPI">
		<rdfs:subClassOf rdf:resource="&java;JavaAPI"/>
		<rdfs:comment xml:lang="en">JavaLibrary implementing the javax.imageio.plugins.bmp package for J2SE 5.0</rdfs:comment>
		<rdfs:comment xml:lang="OWLManchester">platform:comprisesInterfacePart some JavaxImageioPluginsBmp</rdfs:comment>
	</owl:Class>
	<owl:Class rdf:about="&j2se-5_0;JavaxImageioPluginsJpegAPI">
		<owl:equivalentClass rdf:resource="&j2se-1_4;JavaxImageioPluginsJpegAPI"/>
		<rdfs:subClassOf rdf:resource="&java;JavaAPI"/>
		<rdfs:comment xml:lang="en">JavaLibrary implementing the javax.imageio.plugins.jpeg package for J2SE 5.0</rdfs:comment>
		<rdfs:comment xml:lang="OWLManchester">platform:comprisesInterfacePart some JavaxImageioPluginsJpeg</rdfs:comment>
	</owl:Class>
	<owl:Class rdf:about="&j2se-5_0;JavaxImageioStreamAPI">
		<owl:equivalentClass rdf:resource="&j2se-1_4;JavaxImageioStreamAPI"/>
		<rdfs:subClassOf rdf:resource="&java;JavaAPI"/>
		<rdfs:comment xml:lang="en">JavaLibrary implementing the javax.imageio.stream package for J2SE 5.0</rdfs:comment>
		<rdfs:comment xml:lang="OWLManchester">platform:comprisesInterfacePart some JavaxImageioStream</rdfs:comment>
	</owl:Class>
	<owl:Class rdf:about="&j2se-5_0;JavaxImageioSpiAPI">
		<owl:equivalentClass rdf:resource="&j2se-1_4;JavaxImageioSpiAPI"/>
		<rdfs:subClassOf rdf:resource="&java;JavaAPI"/>
		<rdfs:comment xml:lang="en">JavaLibrary implementing the javax.imageio.spi package for J2SE 5.0</rdfs:comment>
		<rdfs:comment xml:lang="OWLManchester">platform:comprisesInterfacePart some JavaxImageioSpi</rdfs:comment>
	</owl:Class>
	<owl:Class rdf:about="&j2se-5_0;JavaxNamingAPI">
		<rdfs:subClassOf rdf:resource="&j2se-1_4;JavaxNamingAPI"/>
		<rdfs:comment xml:lang="en">JavaLibrary implementing the javax.naming package for J2SE 5.0</rdfs:comment>
		<rdfs:comment xml:lang="OWLManchester">platform:comprisesInterfacePart some JavaxNaming</rdfs:comment>
	</owl:Class>
	<owl:Class rdf:about="&j2se-5_0;JavaxNamingDirectoryAPI">
		<rdfs:subClassOf rdf:resource="&j2se-1_4;JavaxNamingDirectoryAPI"/>
		<rdfs:comment xml:lang="en">JavaLibrary implementing the javax.naming.directory package for J2SE 5.0</rdfs:comment>
		<rdfs:comment xml:lang="OWLManchester">platform:comprisesInterfacePart some JavaxNamingDirectory</rdfs:comment>
	</owl:Class>
	<owl:Class rdf:about="&j2se-5_0;JavaxNamingEventAPI">
		<owl:equivalentClass rdf:resource="&j2se-1_4;JavaxNamingEventAPI"/>
		<rdfs:subClassOf rdf:resource="&java;JavaAPI"/>
		<rdfs:comment xml:lang="en">JavaLibrary implementing the javax.naming.event package for J2SE 5.0</rdfs:comment>
		<rdfs:comment xml:lang="OWLManchester">platform:comprisesInterfacePart some JavaxNamingEvent</rdfs:comment>
	</owl:Class>
	<owl:Class rdf:about="&j2se-5_0;JavaxNamingLdapAPI">
		<rdfs:subClassOf rdf:resource="&j2se-1_4;JavaxNamingLdapAPI"/>
		<rdfs:comment xml:lang="en">JavaLibrary implementing the javax.naming.ldap package for J2SE 5.0</rdfs:comment>
		<rdfs:comment xml:lang="OWLManchester">platform:comprisesInterfacePart some JavaxNamingLdap</rdfs:comment>
	</owl:Class>
	<owl:Class rdf:about="&j2se-5_0;JavaxNamingSpiAPI">
		<owl:equivalentClass rdf:resource="&j2se-1_4;JavaxNamingSpiAPI"/>
		<rdfs:subClassOf rdf:resource="&java;JavaAPI"/>
		<rdfs:comment xml:lang="en">JavaLibrary implementing the javax.naming.spi package for J2SE 5.0</rdfs:comment>
		<rdfs:comment xml:lang="OWLManchester">platform:comprisesInterfacePart some JavaxNamingSpi</rdfs:comment>
	</owl:Class>
	<owl:Class rdf:about="&j2se-5_0;JavaxPrintAPI">
		<owl:equivalentClass rdf:resource="&j2se-1_4;JavaxPrintAPI"/>
		<rdfs:subClassOf rdf:resource="&java;JavaAPI"/>
		<rdfs:comment xml:lang="en">JavaLibrary implementing the javax.print package for J2SE 5.0</rdfs:comment>
		<rdfs:comment xml:lang="OWLManchester">platform:comprisesInterfacePart some JavaxPrint</rdfs:comment>
	</owl:Class>
	<owl:Class rdf:about="&j2se-5_0;JavaxPrintAttributeAPI">
		<owl:equivalentClass rdf:resource="&j2se-1_4;JavaxPrintAttributeAPI"/>
		<rdfs:subClassOf rdf:resource="&java;JavaAPI"/>
		<rdfs:comment xml:lang="en">JavaLibrary implementing the javax.print.attribute package for J2SE 5.0</rdfs:comment>
		<rdfs:comment xml:lang="OWLManchester">platform:comprisesInterfacePart some JavaxPrintAttribute</rdfs:comment>
	</owl:Class>
	<owl:Class rdf:about="&j2se-5_0;JavaxPrintAttributeStandardAPI">
		<rdfs:subClassOf rdf:resource="&j2se-1_4;JavaxPrintAttributeStandardAPI"/>
		<rdfs:comment xml:lang="en">JavaLibrary implementing the javax.print.attribute.standard package for J2SE 5.0</rdfs:comment>
		<rdfs:comment xml:lang="OWLManchester">platform:comprisesInterfacePart some JavaxPrintAttributeStandard</rdfs:comment>
	</owl:Class>
	<owl:Class rdf:about="&j2se-5_0;JavaxPrintEventAPI">
		<owl:equivalentClass rdf:resource="&j2se-1_4;JavaxPrintEventAPI"/>
		<rdfs:subClassOf rdf:resource="&java;JavaAPI"/>
		<rdfs:comment xml:lang="en">JavaLibrary implementing the javax.print.event package for J2SE 5.0</rdfs:comment>
		<rdfs:comment xml:lang="OWLManchester">platform:comprisesInterfacePart some JavaxPrintEvent</rdfs:comment>
	</owl:Class>
	<owl:Class rdf:about="&j2se-5_0;JavaxRmiAPI">
		<owl:equivalentClass rdf:resource="&j2se-1_4;JavaxRmiAPI"/>
		<rdfs:subClassOf rdf:resource="&java;JavaAPI"/>
		<rdfs:comment xml:lang="en">JavaLibrary implementing the javax.rmi package for J2SE 5.0</rdfs:comment>
		<rdfs:comment xml:lang="OWLManchester">platform:comprisesInterfacePart some JavaxRmi</rdfs:comment>
	</owl:Class>
	<owl:Class rdf:about="&j2se-5_0;JavaxRmiCORBAAPI">
		<rdfs:subClassOf rdf:resource="&j2se-1_4;JavaxRmiCORBAAPI"/>
		<rdfs:comment xml:lang="en">JavaLibrary implementing the javax.rmi.CORBA package for J2SE 5.0</rdfs:comment>
		<rdfs:comment xml:lang="OWLManchester">platform:comprisesInterfacePart some JavaxRmiCORBA</rdfs:comment>
	</owl:Class>
	<owl:Class rdf:about="&j2se-5_0;JavaxRmiSslAPI">
		<rdfs:subClassOf rdf:resource="&java;JavaAPI"/>
		<rdfs:comment xml:lang="en">JavaLibrary implementing the javax.rmi.ssl package for J2SE 5.0</rdfs:comment>
		<rdfs:comment xml:lang="OWLManchester">platform:comprisesInterfacePart some JavaxRmiSsl</rdfs:comment>
	</owl:Class>
	<owl:Class rdf:about="&j2se-5_0;JavaxSoundMidiAPI">
		<rdfs:subClassOf rdf:resource="&java;JavaAPI"/>
		<rdfs:comment xml:lang="en">JavaLibrary implementing the javax.sound.midi package for J2SE 5.0</rdfs:comment>
		<rdfs:comment xml:lang="OWLManchester">platform:comprisesInterfacePart some JavaxSoundMidi</rdfs:comment>
	</owl:Class>
	<owl:Class rdf:about="&j2se-5_0;JavaxSoundMidiSpiAPI">
		<owl:equivalentClass rdf:resource="&j2se-1_4;JavaxSoundMidiSpiAPI"/>
		<rdfs:subClassOf rdf:resource="&java;JavaAPI"/>
		<rdfs:comment xml:lang="en">JavaLibrary implementing the javax.sound.midi.spi package for J2SE 5.0</rdfs:comment>
		<rdfs:comment xml:lang="OWLManchester">platform:comprisesInterfacePart some JavaxSoundMidiSpi</rdfs:comment>
	</owl:Class>
	<owl:Class rdf:about="&j2se-5_0;JavaxSoundSampledAPI">
		<rdfs:subClassOf rdf:resource="&j2se-1_4;JavaxSoundSampledAPI"/>
		<rdfs:comment xml:lang="en">JavaLibrary implementing the javax.sound.sampled package for J2SE 5.0</rdfs:comment>
		<rdfs:comment xml:lang="OWLManchester">platform:comprisesInterfacePart some JavaxSoundSampled</rdfs:comment>
	</owl:Class>
	<owl:Class rdf:about="&j2se-5_0;JavaxSoundSampledSpiAPI">
		<owl:equivalentClass rdf:resource="&j2se-1_4;JavaxSoundSampledSpiAPI"/>
		<rdfs:subClassOf rdf:resource="&java;JavaAPI"/>
		<rdfs:comment xml:lang="en">JavaLibrary implementing the javax.sound.sampled.spi package for J2SE 5.0</rdfs:comment>
		<rdfs:comment xml:lang="OWLManchester">platform:comprisesInterfacePart some JavaxSoundSampledSpi</rdfs:comment>
	</owl:Class>
	<owl:Class rdf:about="&j2se-5_0;JavaxSqlAPI">
		<owl:equivalentClass rdf:resource="&j2se-1_4;JavaxSqlAPI"/>
		<rdfs:subClassOf rdf:resource="&java;JavaAPI"/>
		<rdfs:comment xml:lang="en">JavaLibrary implementing the javax.sql package for J2SE 5.0</rdfs:comment>
		<rdfs:comment xml:lang="OWLManchester">platform:comprisesInterfacePart some JavaxSql</rdfs:comment>
	</owl:Class>
	<owl:Class rdf:about="&j2se-5_0;JavaxSqlRowsetAPI">
		<rdfs:subClassOf rdf:resource="&java;JavaAPI"/>
		<rdfs:comment xml:lang="en">JavaLibrary implementing the javax.sql.rowset package for J2SE 5.0</rdfs:comment>
		<rdfs:comment xml:lang="OWLManchester">platform:comprisesInterfacePart some JavaxSqlRowset</rdfs:comment>
	</owl:Class>
	<owl:Class rdf:about="&j2se-5_0;JavaxSqlRowsetSpiAPI">
		<rdfs:subClassOf rdf:resource="&java;JavaAPI"/>
		<rdfs:comment xml:lang="en">JavaLibrary implementing the javax.sql.rowset.spi package for J2SE 5.0</rdfs:comment>
		<rdfs:comment xml:lang="OWLManchester">platform:comprisesInterfacePart some JavaxSqlRowsetSpi</rdfs:comment>
	</owl:Class>
	<owl:Class rdf:about="&j2se-5_0;JavaxSqlRowsetSerialAPI">
		<rdfs:subClassOf rdf:resource="&java;JavaAPI"/>
		<rdfs:comment xml:lang="en">JavaLibrary implementing the javax.sql.rowset.serial package for J2SE 5.0</rdfs:comment>
		<rdfs:comment xml:lang="OWLManchester">platform:comprisesInterfacePart some JavaxSqlRowsetSerial</rdfs:comment>
	</owl:Class>
	<owl:Class rdf:about="&j2se-5_0;JavaxTransactionAPI">
		<owl:equivalentClass rdf:resource="&j2se-1_4;JavaxTransactionAPI"/>
		<rdfs:subClassOf rdf:resource="&java;JavaAPI"/>
		<rdfs:comment xml:lang="en">JavaLibrary implementing the javax.transaction package for J2SE 5.0</rdfs:comment>
		<rdfs:comment xml:lang="OWLManchester">platform:comprisesInterfacePart some JavaxTransaction</rdfs:comment>
	</owl:Class>
	<owl:Class rdf:about="&j2se-5_0;JavaxTransactionXaAPI">
		<owl:equivalentClass rdf:resource="&j2se-1_4;JavaxTransactionXaAPI"/>
		<rdfs:subClassOf rdf:resource="&java;JavaAPI"/>
		<rdfs:comment xml:lang="en">JavaLibrary implementing the javax.transaction.xa package for J2SE 5.0</rdfs:comment>
		<rdfs:comment xml:lang="OWLManchester">platform:comprisesInterfacePart some JavaxTransactionXa</rdfs:comment>
	</owl:Class>
	<owl:Class rdf:about="&j2se-5_0;JavaxXmlAPI">
		<rdfs:subClassOf rdf:resource="&java;JavaAPI"/>
		<rdfs:comment xml:lang="en">JavaLibrary implementing the javax.xml package for J2SE 5.0</rdfs:comment>
		<rdfs:comment xml:lang="OWLManchester">platform:comprisesInterfacePart some JavaxXml</rdfs:comment>
	</owl:Class>
	<owl:Class rdf:about="&j2se-5_0;JavaxXmlDatatypeAPI">
		<rdfs:subClassOf rdf:resource="&java;JavaAPI"/>
		<rdfs:comment xml:lang="en">JavaLibrary implementing the javax.xml.datatype package for J2SE 5.0</rdfs:comment>
		<rdfs:comment xml:lang="OWLManchester">platform:comprisesInterfacePart some JavaxXmlDatatype</rdfs:comment>
	</owl:Class>
	<owl:Class rdf:about="&j2se-5_0;JavaxXmlNamespaceAPI">
		<rdfs:subClassOf rdf:resource="&java;JavaAPI"/>
		<rdfs:comment xml:lang="en">JavaLibrary implementing the javax.xml.namespace package for J2SE 5.0</rdfs:comment>
		<rdfs:comment xml:lang="OWLManchester">platform:comprisesInterfacePart some JavaxXmlNamespace</rdfs:comment>
	</owl:Class>
	<owl:Class rdf:about="&j2se-5_0;JavaxXmlTransformAPI">
		<rdfs:subClassOf rdf:resource="&j2se-1_4;JavaxXmlTransformAPI"/>
		<rdfs:comment xml:lang="en">JavaLibrary implementing the javax.xml.transform package for J2SE 5.0</rdfs:comment>
		<rdfs:comment xml:lang="OWLManchester">platform:comprisesInterfacePart some JavaxXmlTransform</rdfs:comment>
	</owl:Class>
	<owl:Class rdf:about="&j2se-5_0;JavaxXmlTransformDomAPI">
		<rdfs:subClassOf rdf:resource="&j2se-1_4;JavaxXmlTransformDomAPI"/>
		<rdfs:comment xml:lang="en">JavaLibrary implementing the javax.xml.transform.dom package for J2SE 5.0</rdfs:comment>
		<rdfs:comment xml:lang="OWLManchester">platform:comprisesInterfacePart some JavaxXmlTransformDom</rdfs:comment>
	</owl:Class>
	<owl:Class rdf:about="&j2se-5_0;JavaxXmlTransformSaxAPI">
		<rdfs:subClassOf rdf:resource="&j2se-1_4;JavaxXmlTransformSaxAPI"/>
		<rdfs:comment xml:lang="en">JavaLibrary implementing the javax.xml.transform.sax package for J2SE 5.0</rdfs:comment>
		<rdfs:comment xml:lang="OWLManchester">platform:comprisesInterfacePart some JavaxXmlTransformSax</rdfs:comment>
	</owl:Class>
	<owl:Class rdf:about="&j2se-5_0;JavaxXmlTransformStreamAPI">
		<owl:equivalentClass rdf:resource="&j2se-1_4;JavaxXmlTransformStreamAPI"/>
		<rdfs:subClassOf rdf:resource="&java;JavaAPI"/>
		<rdfs:comment xml:lang="en">JavaLibrary implementing the javax.xml.transform.stream package for J2SE 5.0</rdfs:comment>
		<rdfs:comment xml:lang="OWLManchester">platform:comprisesInterfacePart some JavaxXmlTransformStream</rdfs:comment>
	</owl:Class>
	<owl:Class rdf:about="&j2se-5_0;JavaxXmlValidationAPI">
		<rdfs:subClassOf rdf:resource="&java;JavaAPI"/>
		<rdfs:comment xml:lang="en">JavaLibrary implementing the javax.xml.validation package for J2SE 5.0</rdfs:comment>
		<rdfs:comment xml:lang="OWLManchester">platform:comprisesInterfacePart some JavaxXmlValidation</rdfs:comment>
	</owl:Class>
	<owl:Class rdf:about="&j2se-5_0;JavaxXmlXpathAPI">
		<rdfs:subClassOf rdf:resource="&java;JavaAPI"/>
		<rdfs:comment xml:lang="en">JavaLibrary implementing the javax.xml.xpath package for J2SE 5.0</rdfs:comment>
		<rdfs:comment xml:lang="OWLManchester">platform:comprisesInterfacePart some JavaxXmlXpath</rdfs:comment>
	</owl:Class>
	<owl:Class rdf:about="&j2se-5_0;JavaxXmlParsersAPI">
		<rdfs:subClassOf rdf:resource="&j2se-1_4;JavaxXmlParsersAPI"/>
		<rdfs:comment xml:lang="en">JavaLibrary implementing the javax.xml.parsers package for J2SE 5.0</rdfs:comment>
		<rdfs:comment xml:lang="OWLManchester">platform:comprisesInterfacePart some JavaxXmlParsers</rdfs:comment>
	</owl:Class>
	<owl:Class rdf:about="&j2se-5_0;JavaLangAPI">
		<rdfs:subClassOf rdf:resource="&j2se-1_4;JavaLangAPI"/>
		<rdfs:comment xml:lang="en">JavaLibrary implementing the java.lang package for J2SE 5.0</rdfs:comment>
		<rdfs:comment xml:lang="OWLManchester">platform:comprisesInterfacePart some JavaLang</rdfs:comment>
	</owl:Class>
	<owl:Class rdf:about="&j2se-5_0;JavaLangReflectAPI">
		<rdfs:subClassOf rdf:resource="&j2se-1_4;JavaLangReflectAPI"/>
		<rdfs:comment xml:lang="en">JavaLibrary implementing the java.lang.reflect package for J2SE 5.0</rdfs:comment>
		<rdfs:comment xml:lang="OWLManchester">platform:comprisesInterfacePart some JavaLangReflect</rdfs:comment>
	</owl:Class>
	<owl:Class rdf:about="&j2se-5_0;JavaLangAnnotationAPI">
		<rdfs:subClassOf rdf:resource="&java;JavaAPI"/>
		<rdfs:comment xml:lang="en">JavaLibrary implementing the java.lang.annotation package for J2SE 5.0</rdfs:comment>
		<rdfs:comment xml:lang="OWLManchester">platform:comprisesInterfacePart some JavaLangAnnotation</rdfs:comment>
	</owl:Class>
	<owl:Class rdf:about="&j2se-5_0;JavaLangInstrumentAPI">
		<rdfs:subClassOf rdf:resource="&java;JavaAPI"/>
		<rdfs:comment xml:lang="en">JavaLibrary implementing the java.lang.instrument package for J2SE 5.0</rdfs:comment>
		<rdfs:comment xml:lang="OWLManchester">platform:comprisesInterfacePart some JavaLangInstrument</rdfs:comment>
	</owl:Class>
	<owl:Class rdf:about="&j2se-5_0;JavaLangManagementAPI">
		<rdfs:subClassOf rdf:resource="&java;JavaAPI"/>
		<rdfs:comment xml:lang="en">JavaLibrary implementing the java.lang.management package for J2SE 5.0</rdfs:comment>
		<rdfs:comment xml:lang="OWLManchester">platform:comprisesInterfacePart some JavaLangManagement</rdfs:comment>
	</owl:Class>
	<owl:Class rdf:about="&j2se-5_0;JavaLangRefAPI">
		<owl:equivalentClass rdf:resource="&j2se-1_4;JavaLangRefAPI"/>
		<rdfs:subClassOf rdf:resource="&java;JavaAPI"/>
		<rdfs:comment xml:lang="en">JavaLibrary implementing the java.lang.ref package for J2SE 5.0</rdfs:comment>
		<rdfs:comment xml:lang="OWLManchester">platform:comprisesInterfacePart some JavaLangRef</rdfs:comment>
	</owl:Class>
	<owl:Class rdf:about="&j2se-5_0;JavaSecurityAPI">
		<rdfs:subClassOf rdf:resource="&j2se-1_4;JavaSecurityAPI"/>
		<rdfs:comment xml:lang="en">JavaLibrary implementing the java.security package for J2SE 5.0</rdfs:comment>
		<rdfs:comment xml:lang="OWLManchester">platform:comprisesInterfacePart some JavaSecurity</rdfs:comment>
	</owl:Class>
	<owl:Class rdf:about="&j2se-5_0;JavaSecuritySpecAPI">
		<rdfs:subClassOf rdf:resource="&j2se-1_4;JavaSecuritySpecAPI"/>
		<rdfs:comment xml:lang="en">JavaLibrary implementing the java.security.spec package for J2SE 5.0</rdfs:comment>
		<rdfs:comment xml:lang="OWLManchester">platform:comprisesInterfacePart some JavaSecuritySpec</rdfs:comment>
	</owl:Class>
	<owl:Class rdf:about="&j2se-5_0;JavaSecurityCertAPI">
		<rdfs:subClassOf rdf:resource="&java;JavaAPI"/>
		<rdfs:comment xml:lang="en">JavaLibrary implementing the java.security.cert package for J2SE 5.0</rdfs:comment>
		<rdfs:comment xml:lang="OWLManchester">platform:comprisesInterfacePart some JavaSecurityCert</rdfs:comment>
	</owl:Class>
	<owl:Class rdf:about="&j2se-5_0;JavaSecurityAclAPI">
		<owl:equivalentClass rdf:resource="&j2se-1_4;JavaSecurityAclAPI"/>
		<rdfs:subClassOf rdf:resource="&java;JavaAPI"/>
		<rdfs:comment xml:lang="en">JavaLibrary implementing the java.security.acl package for J2SE 5.0</rdfs:comment>
		<rdfs:comment xml:lang="OWLManchester">platform:comprisesInterfacePart some JavaSecurityAcl</rdfs:comment>
	</owl:Class>
	<owl:Class rdf:about="&j2se-5_0;JavaSecurityInterfacesAPI">
		<rdfs:subClassOf rdf:resource="&j2se-1_4;JavaSecurityInterfacesAPI"/>
		<rdfs:comment xml:lang="en">JavaLibrary implementing the java.security.interfaces package for J2SE 5.0</rdfs:comment>
		<rdfs:comment xml:lang="OWLManchester">platform:comprisesInterfacePart some JavaSecurityInterfaces</rdfs:comment>
	</owl:Class>
	<owl:Class rdf:about="&j2se-5_0;JavaMathAPI">
		<rdfs:subClassOf rdf:resource="&j2se-1_4;JavaMathAPI"/>
		<rdfs:comment xml:lang="en">JavaLibrary implementing the java.math package for J2SE 5.0</rdfs:comment>
		<rdfs:comment xml:lang="OWLManchester">platform:comprisesInterfacePart some JavaMath</rdfs:comment>
	</owl:Class>
	<owl:Class rdf:about="&j2se-5_0;JavaNioAPI">
		<rdfs:subClassOf rdf:resource="&j2se-1_4;JavaNioAPI"/>
		<rdfs:comment xml:lang="en">JavaLibrary implementing the java.nio package for J2SE 5.0</rdfs:comment>
		<rdfs:comment xml:lang="OWLManchester">platform:comprisesInterfacePart some JavaNio</rdfs:comment>
	</owl:Class>
	<owl:Class rdf:about="&j2se-5_0;JavaNioChannelsAPI">
		<rdfs:subClassOf rdf:resource="&j2se-1_4;JavaNioChannelsAPI"/>
		<rdfs:comment xml:lang="en">JavaLibrary implementing the java.nio.channels package for J2SE 5.0</rdfs:comment>
		<rdfs:comment xml:lang="OWLManchester">platform:comprisesInterfacePart some JavaNioChannels</rdfs:comment>
	</owl:Class>
	<owl:Class rdf:about="&j2se-5_0;JavaNioChannelsSpiAPI">
		<rdfs:subClassOf rdf:resource="&j2se-1_4;JavaNioChannelsSpiAPI"/>
		<rdfs:comment xml:lang="en">JavaLibrary implementing the java.nio.channels.spi package for J2SE 5.0</rdfs:comment>
		<rdfs:comment xml:lang="OWLManchester">platform:comprisesInterfacePart some JavaNioChannelsSpi</rdfs:comment>
	</owl:Class>
	<owl:Class rdf:about="&j2se-5_0;JavaNioCharsetAPI">
		<rdfs:subClassOf rdf:resource="&j2se-1_4;JavaNioCharsetAPI"/>
		<rdfs:comment xml:lang="en">JavaLibrary implementing the java.nio.charset package for J2SE 5.0</rdfs:comment>
		<rdfs:comment xml:lang="OWLManchester">platform:comprisesInterfacePart some JavaNioCharset</rdfs:comment>
	</owl:Class>
	<owl:Class rdf:about="&j2se-5_0;JavaNioCharsetSpiAPI">
		<owl:equivalentClass rdf:resource="&j2se-1_4;JavaNioCharsetSpiAPI"/>
		<rdfs:subClassOf rdf:resource="&java;JavaAPI"/>
		<rdfs:comment xml:lang="en">JavaLibrary implementing the java.nio.charset.spi package for J2SE 5.0</rdfs:comment>
		<rdfs:comment xml:lang="OWLManchester">platform:comprisesInterfacePart some JavaNioCharsetSpi</rdfs:comment>
	</owl:Class>
	<owl:Class rdf:about="&j2se-5_0;JavaIoAPI">
		<rdfs:subClassOf rdf:resource="&j2se-1_4;JavaIoAPI"/>
		<rdfs:comment xml:lang="en">JavaLibrary implementing the java.io package for J2SE 5.0</rdfs:comment>
		<rdfs:comment xml:lang="OWLManchester">platform:comprisesInterfacePart some JavaIo</rdfs:comment>
	</owl:Class>
	<owl:Class rdf:about="&j2se-5_0;JavaNetAPI">
		<rdfs:subClassOf rdf:resource="&j2se-1_4;JavaNetAPI"/>
		<rdfs:comment xml:lang="en">JavaLibrary implementing the java.net package for J2SE 5.0</rdfs:comment>
		<rdfs:comment xml:lang="OWLManchester">platform:comprisesInterfacePart some JavaNet</rdfs:comment>
	</owl:Class>
	<owl:Class rdf:about="&j2se-5_0;JavaUtilAPI">
		<rdfs:subClassOf rdf:resource="&j2se-1_4;JavaUtilAPI"/>
		<rdfs:comment xml:lang="en">JavaLibrary implementing the java.util package for J2SE 5.0</rdfs:comment>
		<rdfs:comment xml:lang="OWLManchester">platform:comprisesInterfacePart some JavaUtil</rdfs:comment>
	</owl:Class>
	<owl:Class rdf:about="&j2se-5_0;JavaUtilRegexAPI">
		<rdfs:subClassOf rdf:resource="&j2se-1_4;JavaUtilRegexAPI"/>
		<rdfs:comment xml:lang="en">JavaLibrary implementing the java.util.regex package for J2SE 5.0</rdfs:comment>
		<rdfs:comment xml:lang="OWLManchester">platform:comprisesInterfacePart some JavaUtilRegex</rdfs:comment>
	</owl:Class>
	<owl:Class rdf:about="&j2se-5_0;JavaUtilConcurrentAPI">
		<rdfs:subClassOf rdf:resource="&java;JavaAPI"/>
		<rdfs:comment xml:lang="en">JavaLibrary implementing the java.util.concurrent package for J2SE 5.0</rdfs:comment>
		<rdfs:comment xml:lang="OWLManchester">platform:comprisesInterfacePart some JavaUtilConcurrent</rdfs:comment>
	</owl:Class>
	<owl:Class rdf:about="&j2se-5_0;JavaUtilConcurrentAtomicAPI">
		<rdfs:subClassOf rdf:resource="&java;JavaAPI"/>
		<rdfs:comment xml:lang="en">JavaLibrary implementing the java.util.concurrent.atomic package for J2SE 5.0</rdfs:comment>
		<rdfs:comment xml:lang="OWLManchester">platform:comprisesInterfacePart some JavaUtilConcurrentAtomic</rdfs:comment>
	</owl:Class>
	<owl:Class rdf:about="&j2se-5_0;JavaUtilConcurrentLocksAPI">
		<rdfs:subClassOf rdf:resource="&java;JavaAPI"/>
		<rdfs:comment xml:lang="en">JavaLibrary implementing the java.util.concurrent.locks package for J2SE 5.0</rdfs:comment>
		<rdfs:comment xml:lang="OWLManchester">platform:comprisesInterfacePart some JavaUtilConcurrentLocks</rdfs:comment>
	</owl:Class>
	<owl:Class rdf:about="&j2se-5_0;JavaUtilJarAPI">
		<rdfs:subClassOf rdf:resource="&j2se-1_4;JavaUtilJarAPI"/>
		<rdfs:comment xml:lang="en">JavaLibrary implementing the java.util.jar package for J2SE 5.0</rdfs:comment>
		<rdfs:comment xml:lang="OWLManchester">platform:comprisesInterfacePart some JavaUtilJar</rdfs:comment>
	</owl:Class>
	<owl:Class rdf:about="&j2se-5_0;JavaUtilZipAPI">
		<rdfs:subClassOf rdf:resource="&j2se-1_4;JavaUtilZipAPI"/>
		<rdfs:comment xml:lang="en">JavaLibrary implementing the java.util.zip package for J2SE 5.0</rdfs:comment>
		<rdfs:comment xml:lang="OWLManchester">platform:comprisesInterfacePart some JavaUtilZip</rdfs:comment>
	</owl:Class>
	<owl:Class rdf:about="&j2se-5_0;JavaUtilLoggingAPI">
		<rdfs:subClassOf rdf:resource="&j2se-1_4;JavaUtilLoggingAPI"/>
		<rdfs:comment xml:lang="en">JavaLibrary implementing the java.util.logging package for J2SE 5.0</rdfs:comment>
		<rdfs:comment xml:lang="OWLManchester">platform:comprisesInterfacePart some JavaUtilLogging</rdfs:comment>
	</owl:Class>
	<owl:Class rdf:about="&j2se-5_0;JavaUtilPrefsAPI">
		<owl:equivalentClass rdf:resource="&j2se-1_4;JavaUtilPrefsAPI"/>
		<rdfs:subClassOf rdf:resource="&java;JavaAPI"/>
		<rdfs:comment xml:lang="en">JavaLibrary implementing the java.util.prefs package for J2SE 5.0</rdfs:comment>
		<rdfs:comment xml:lang="OWLManchester">platform:comprisesInterfacePart some JavaUtilPrefs</rdfs:comment>
	</owl:Class>
	<owl:Class rdf:about="&j2se-5_0;JavaAppletAPI">
		<rdfs:subClassOf rdf:resource="&j2se-1_4;JavaAppletAPI"/>
		<rdfs:comment xml:lang="en">JavaLibrary implementing the java.applet package for J2SE 5.0</rdfs:comment>
		<rdfs:comment xml:lang="OWLManchester">platform:comprisesInterfacePart some JavaApplet</rdfs:comment>
	</owl:Class>
	<owl:Class rdf:about="&j2se-5_0;JavaAwtAPI">
		<rdfs:subClassOf rdf:resource="&j2se-1_4;JavaAwtAPI"/>
		<rdfs:comment xml:lang="en">JavaLibrary implementing the java.awt package for J2SE 5.0</rdfs:comment>
		<rdfs:comment xml:lang="OWLManchester">platform:comprisesInterfacePart some JavaAwt</rdfs:comment>
	</owl:Class>
	<owl:Class rdf:about="&j2se-5_0;JavaAwtEventAPI">
		<rdfs:subClassOf rdf:resource="&j2se-1_4;JavaAwtEventAPI"/>
		<rdfs:comment xml:lang="en">JavaLibrary implementing the java.awt.event package for J2SE 5.0</rdfs:comment>
		<rdfs:comment xml:lang="OWLManchester">platform:comprisesInterfacePart some JavaAwtEvent</rdfs:comment>
	</owl:Class>
	<owl:Class rdf:about="&j2se-5_0;JavaAwtImageAPI">
		<rdfs:subClassOf rdf:resource="&j2se-1_4;JavaAwtImageAPI"/>
		<rdfs:comment xml:lang="en">JavaLibrary implementing the java.awt.image package for J2SE 5.0</rdfs:comment>
		<rdfs:comment xml:lang="OWLManchester">platform:comprisesInterfacePart some JavaAwtImage</rdfs:comment>
	</owl:Class>
	<owl:Class rdf:about="&j2se-5_0;JavaAwtImageRenderableAPI">
		<owl:equivalentClass rdf:resource="&j2se-1_4;JavaAwtImageRenderableAPI"/>
		<rdfs:subClassOf rdf:resource="&java;JavaAPI"/>
		<rdfs:comment xml:lang="en">JavaLibrary implementing the java.awt.image.renderable package for J2SE 5.0</rdfs:comment>
		<rdfs:comment xml:lang="OWLManchester">platform:comprisesInterfacePart some JavaAwtImageRenderable</rdfs:comment>
	</owl:Class>
	<owl:Class rdf:about="&j2se-5_0;JavaAwtGeomAPI">
		<owl:equivalentClass rdf:resource="&j2se-1_4;JavaAwtGeomAPI"/>
		<rdfs:subClassOf rdf:resource="&java;JavaAPI"/>
		<rdfs:comment xml:lang="en">JavaLibrary implementing the java.awt.geom package for J2SE 5.0</rdfs:comment>
		<rdfs:comment xml:lang="OWLManchester">platform:comprisesInterfacePart some JavaAwtGeom</rdfs:comment>
	</owl:Class>
	<owl:Class rdf:about="&j2se-5_0;JavaAwtImAPI">
		<owl:equivalentClass rdf:resource="&j2se-1_4;JavaAwtImAPI"/>
		<rdfs:subClassOf rdf:resource="&java;JavaAPI"/>
		<rdfs:comment xml:lang="en">JavaLibrary implementing the java.awt.im package for J2SE 5.0</rdfs:comment>
		<rdfs:comment xml:lang="OWLManchester">platform:comprisesInterfacePart some JavaAwtIm</rdfs:comment>
	</owl:Class>
	<owl:Class rdf:about="&j2se-5_0;JavaAwtImSpiAPI">
		<owl:equivalentClass rdf:resource="&j2se-1_4;JavaAwtImSpiAPI"/>
		<rdfs:subClassOf rdf:resource="&java;JavaAPI"/>
		<rdfs:comment xml:lang="en">JavaLibrary implementing the java.awt.im.spi package for J2SE 5.0</rdfs:comment>
		<rdfs:comment xml:lang="OWLManchester">platform:comprisesInterfacePart some JavaAwtImSpi</rdfs:comment>
	</owl:Class>
	<owl:Class rdf:about="&j2se-5_0;JavaAwtColorAPI">
		<rdfs:subClassOf rdf:resource="&j2se-1_4;JavaAwtColorAPI"/>
		<rdfs:comment xml:lang="en">JavaLibrary implementing the java.awt.color package for J2SE 5.0</rdfs:comment>
		<rdfs:comment xml:lang="OWLManchester">platform:comprisesInterfacePart some JavaAwtColor</rdfs:comment>
	</owl:Class>
	<owl:Class rdf:about="&j2se-5_0;JavaAwtDatatransferAPI">
		<rdfs:subClassOf rdf:resource="&j2se-1_4;JavaAwtDatatransferAPI"/>
		<rdfs:comment xml:lang="en">JavaLibrary implementing the java.awt.datatransfer package for J2SE 5.0</rdfs:comment>
		<rdfs:comment xml:lang="OWLManchester">platform:comprisesInterfacePart some JavaAwtDatatransfer</rdfs:comment>
	</owl:Class>
	<owl:Class rdf:about="&j2se-5_0;JavaAwtDndAPI">
		<rdfs:subClassOf rdf:resource="&j2se-1_4;JavaAwtDndAPI"/>
		<rdfs:comment xml:lang="en">JavaLibrary implementing the java.awt.dnd package for J2SE 5.0</rdfs:comment>
		<rdfs:comment xml:lang="OWLManchester">platform:comprisesInterfacePart some JavaAwtDnd</rdfs:comment>
	</owl:Class>
	<owl:Class rdf:about="&j2se-5_0;JavaAwtFontAPI">
		<owl:equivalentClass rdf:resource="&j2se-1_4;JavaAwtFontAPI"/>
		<rdfs:subClassOf rdf:resource="&java;JavaAPI"/>
		<rdfs:comment xml:lang="en">JavaLibrary implementing the java.awt.font package for J2SE 5.0</rdfs:comment>
		<rdfs:comment xml:lang="OWLManchester">platform:comprisesInterfacePart some JavaAwtFont</rdfs:comment>
	</owl:Class>
	<owl:Class rdf:about="&j2se-5_0;JavaAwtPrintAPI">
		<owl:equivalentClass rdf:resource="&j2se-1_4;JavaAwtPrintAPI"/>
		<rdfs:subClassOf rdf:resource="&java;JavaAPI"/>
		<rdfs:comment xml:lang="en">JavaLibrary implementing the java.awt.print package for J2SE 5.0</rdfs:comment>
		<rdfs:comment xml:lang="OWLManchester">platform:comprisesInterfacePart some JavaAwtPrint</rdfs:comment>
	</owl:Class>
	<owl:Class rdf:about="&j2se-5_0;JavaTextAPI">
		<rdfs:subClassOf rdf:resource="&j2se-1_4;JavaTextAPI"/>
		<rdfs:comment xml:lang="en">JavaLibrary implementing the java.text package for J2SE 5.0</rdfs:comment>
		<rdfs:comment xml:lang="OWLManchester">platform:comprisesInterfacePart some JavaText</rdfs:comment>
	</owl:Class>
	<owl:Class rdf:about="&j2se-5_0;JavaBeansAPI">
		<rdfs:subClassOf rdf:resource="&j2se-1_4;JavaBeansAPI"/>
		<rdfs:comment xml:lang="en">JavaLibrary implementing the java.beans package for J2SE 5.0</rdfs:comment>
		<rdfs:comment xml:lang="OWLManchester">platform:comprisesInterfacePart some JavaBeans</rdfs:comment>
	</owl:Class>
	<owl:Class rdf:about="&j2se-5_0;JavaBeansBeancontextAPI">
		<owl:equivalentClass rdf:resource="&j2se-1_4;JavaBeansBeancontextAPI"/>
		<rdfs:subClassOf rdf:resource="&java;JavaAPI"/>
		<rdfs:comment xml:lang="en">JavaLibrary implementing the java.beans.beancontext package for J2SE 5.0</rdfs:comment>
		<rdfs:comment xml:lang="OWLManchester">platform:comprisesInterfacePart some JavaBeansBeancontext</rdfs:comment>
	</owl:Class>
	<owl:Class rdf:about="&j2se-5_0;JavaRmiAPI">
		<owl:equivalentClass rdf:resource="&j2se-1_4;JavaRmiAPI"/>
		<rdfs:subClassOf rdf:resource="&java;JavaAPI"/>
		<rdfs:comment xml:lang="en">JavaLibrary implementing the java.rmi package for J2SE 5.0</rdfs:comment>
		<rdfs:comment xml:lang="OWLManchester">platform:comprisesInterfacePart some JavaRmi</rdfs:comment>
	</owl:Class>
	<owl:Class rdf:about="&j2se-5_0;JavaRmiActivationAPI">
		<owl:equivalentClass rdf:resource="&j2se-1_4;JavaRmiActivationAPI"/>
		<rdfs:subClassOf rdf:resource="&java;JavaAPI"/>
		<rdfs:comment xml:lang="en">JavaLibrary implementing the java.rmi.activation package for J2SE 5.0</rdfs:comment>
		<rdfs:comment xml:lang="OWLManchester">platform:comprisesInterfacePart some JavaRmiActivation</rdfs:comment>
	</owl:Class>
	<owl:Class rdf:about="&j2se-5_0;JavaRmiServerAPI">
		<rdfs:subClassOf rdf:resource="&j2se-1_4;JavaRmiServerAPI"/>
		<rdfs:comment xml:lang="en">JavaLibrary implementing the java.rmi.server package for J2SE 5.0</rdfs:comment>
		<rdfs:comment xml:lang="OWLManchester">platform:comprisesInterfacePart some JavaRmiServer</rdfs:comment>
	</owl:Class>
	<owl:Class rdf:about="&j2se-5_0;JavaRmiDgcAPI">
		<owl:equivalentClass rdf:resource="&j2se-1_4;JavaRmiDgcAPI"/>
		<rdfs:subClassOf rdf:resource="&java;JavaAPI"/>
		<rdfs:comment xml:lang="en">JavaLibrary implementing the java.rmi.dgc package for J2SE 5.0</rdfs:comment>
		<rdfs:comment xml:lang="OWLManchester">platform:comprisesInterfacePart some JavaRmiDgc</rdfs:comment>
	</owl:Class>
	<owl:Class rdf:about="&j2se-5_0;JavaRmiRegistryAPI">
		<owl:equivalentClass rdf:resource="&j2se-1_4;JavaRmiRegistryAPI"/>
		<rdfs:subClassOf rdf:resource="&java;JavaAPI"/>
		<rdfs:comment xml:lang="en">JavaLibrary implementing the java.rmi.registry package for J2SE 5.0</rdfs:comment>
		<rdfs:comment xml:lang="OWLManchester">platform:comprisesInterfacePart some JavaRmiRegistry</rdfs:comment>
	</owl:Class>
	<owl:Class rdf:about="&j2se-5_0;JavaSqlAPI">
		<owl:equivalentClass rdf:resource="&j2se-1_4;JavaSqlAPI"/>
		<rdfs:subClassOf rdf:resource="&java;JavaAPI"/>
		<rdfs:comment xml:lang="en">JavaLibrary implementing the java.sql package for J2SE 5.0</rdfs:comment>
		<rdfs:comment xml:lang="OWLManchester">platform:comprisesInterfacePart some JavaSql</rdfs:comment>
	</owl:Class>
	<owl:Class rdf:about="&j2se-5_0;OrgW3cDomAPI">
		<rdfs:subClassOf rdf:resource="&j2se-1_4;OrgW3cDomAPI"/>
		<rdfs:comment xml:lang="en">JavaLibrary implementing the org.w3c.dom package for J2SE 5.0</rdfs:comment>
		<rdfs:comment xml:lang="OWLManchester">platform:comprisesInterfacePart some OrgW3cDom</rdfs:comment>
	</owl:Class>
	<owl:Class rdf:about="&j2se-5_0;OrgW3cDomLsAPI">
		<rdfs:subClassOf rdf:resource="&java;JavaAPI"/>
		<rdfs:comment xml:lang="en">JavaLibrary implementing the org.w3c.dom.ls package for J2SE 5.0</rdfs:comment>
		<rdfs:comment xml:lang="OWLManchester">platform:comprisesInterfacePart some OrgW3cDomLs</rdfs:comment>
	</owl:Class>
	<owl:Class rdf:about="&j2se-5_0;OrgW3cDomBootstrapAPI">
		<rdfs:subClassOf rdf:resource="&java;JavaAPI"/>
		<rdfs:comment xml:lang="en">JavaLibrary implementing the org.w3c.dom.bootstrap package for J2SE 5.0</rdfs:comment>
		<rdfs:comment xml:lang="OWLManchester">platform:comprisesInterfacePart some OrgW3cDomBootstrap</rdfs:comment>
	</owl:Class>
	<owl:Class rdf:about="&j2se-5_0;OrgW3cDomCssAPI">
		<rdfs:subClassOf rdf:resource="&j2se-1_4;OrgW3cDomCssAPI"/>
		<rdfs:comment xml:lang="en">JavaLibrary implementing the org.w3c.dom.css package for J2SE 5.0</rdfs:comment>
		<rdfs:comment xml:lang="OWLManchester">platform:comprisesInterfacePart some OrgW3cDomCss</rdfs:comment>
	</owl:Class>
	<owl:Class rdf:about="&j2se-5_0;OrgW3cDomStylesheetsAPI">
		<owl:equivalentClass rdf:resource="&j2se-1_4;OrgW3cDomStylesheetsAPI"/>
		<rdfs:subClassOf rdf:resource="&java;JavaAPI"/>
		<rdfs:comment xml:lang="en">JavaLibrary implementing the org.w3c.dom.stylesheets package for J2SE 5.0</rdfs:comment>
		<rdfs:comment xml:lang="OWLManchester">platform:comprisesInterfacePart some OrgW3cDomStylesheets</rdfs:comment>
	</owl:Class>
	<owl:Class rdf:about="&j2se-5_0;OrgW3cDomViewsAPI">
		<owl:equivalentClass rdf:resource="&j2se-1_4;OrgW3cDomViewsAPI"/>
		<rdfs:subClassOf rdf:resource="&java;JavaAPI"/>
		<rdfs:comment xml:lang="en">JavaLibrary implementing the org.w3c.dom.views package for J2SE 5.0</rdfs:comment>
		<rdfs:comment xml:lang="OWLManchester">platform:comprisesInterfacePart some OrgW3cDomViews</rdfs:comment>
	</owl:Class>
	<owl:Class rdf:about="&j2se-5_0;OrgW3cDomEventsAPI">
		<owl:equivalentClass rdf:resource="&j2se-1_4;OrgW3cDomEventsAPI"/>
		<rdfs:subClassOf rdf:resource="&java;JavaAPI"/>
		<rdfs:comment xml:lang="en">JavaLibrary implementing the org.w3c.dom.events package for J2SE 5.0</rdfs:comment>
		<rdfs:comment xml:lang="OWLManchester">platform:comprisesInterfacePart some OrgW3cDomEvents</rdfs:comment>
	</owl:Class>
	<owl:Class rdf:about="&j2se-5_0;OrgW3cDomHtmlAPI">
		<rdfs:subClassOf rdf:resource="&j2se-1_4;OrgW3cDomHtmlAPI"/>
		<rdfs:comment xml:lang="en">JavaLibrary implementing the org.w3c.dom.html package for J2SE 5.0</rdfs:comment>
		<rdfs:comment xml:lang="OWLManchester">platform:comprisesInterfacePart some OrgW3cDomHtml</rdfs:comment>
	</owl:Class>
	<owl:Class rdf:about="&j2se-5_0;OrgW3cDomTraversalAPI">
		<owl:equivalentClass rdf:resource="&j2se-1_4;OrgW3cDomTraversalAPI"/>
		<rdfs:subClassOf rdf:resource="&java;JavaAPI"/>
		<rdfs:comment xml:lang="en">JavaLibrary implementing the org.w3c.dom.traversal package for J2SE 5.0</rdfs:comment>
		<rdfs:comment xml:lang="OWLManchester">platform:comprisesInterfacePart some OrgW3cDomTraversal</rdfs:comment>
	</owl:Class>
	<owl:Class rdf:about="&j2se-5_0;OrgW3cDomRangesAPI">
		<rdfs:subClassOf rdf:resource="&java;JavaAPI"/>
		<rdfs:comment xml:lang="en">JavaLibrary implementing the org.w3c.dom.ranges package for J2SE 5.0</rdfs:comment>
		<rdfs:comment xml:lang="OWLManchester">platform:comprisesInterfacePart some OrgW3cDomRanges</rdfs:comment>
	</owl:Class>
	<owl:Class rdf:about="&j2se-5_0;OrgOmgCORBA_2_3API">
		<owl:equivalentClass rdf:resource="&j2se-1_4;OrgOmgCORBA_2_3API"/>
		<rdfs:subClassOf rdf:resource="&java;JavaAPI"/>
		<rdfs:comment xml:lang="en">JavaLibrary implementing the org.omg.CORBA_2_3 package for J2SE 5.0</rdfs:comment>
		<rdfs:comment xml:lang="OWLManchester">platform:comprisesInterfacePart some OrgOmgCORBA_2_3</rdfs:comment>
	</owl:Class>
	<owl:Class rdf:about="&j2se-5_0;OrgOmgCORBA_2_3PortableAPI">
		<owl:equivalentClass rdf:resource="&j2se-1_4;OrgOmgCORBA_2_3PortableAPI"/>
		<rdfs:subClassOf rdf:resource="&java;JavaAPI"/>
		<rdfs:comment xml:lang="en">JavaLibrary implementing the org.omg.CORBA_2_3.portable package for J2SE 5.0</rdfs:comment>
		<rdfs:comment xml:lang="OWLManchester">platform:comprisesInterfacePart some OrgOmgCORBA_2_3Portable</rdfs:comment>
	</owl:Class>
	<owl:Class rdf:about="&j2se-5_0;OrgOmgCORBAAPI">
		<rdfs:subClassOf rdf:resource="&j2se-1_4;OrgOmgCORBAAPI"/>
		<rdfs:comment xml:lang="en">JavaLibrary implementing the org.omg.CORBA package for J2SE 5.0</rdfs:comment>
		<rdfs:comment xml:lang="OWLManchester">platform:comprisesInterfacePart some OrgOmgCORBA</rdfs:comment>
	</owl:Class>
	<owl:Class rdf:about="&j2se-5_0;OrgOmgCORBAPortableAPI">
		<rdfs:subClassOf rdf:resource="&j2se-1_4;OrgOmgCORBAPortableAPI"/>
		<rdfs:comment xml:lang="en">JavaLibrary implementing the org.omg.CORBA.portable package for J2SE 5.0</rdfs:comment>
		<rdfs:comment xml:lang="OWLManchester">platform:comprisesInterfacePart some OrgOmgCORBAPortable</rdfs:comment>
	</owl:Class>
	<owl:Class rdf:about="&j2se-5_0;OrgOmgCORBADynAnyPackageAPI">
		<owl:equivalentClass rdf:resource="&j2se-1_4;OrgOmgCORBADynAnyPackageAPI"/>
		<rdfs:subClassOf rdf:resource="&java;JavaAPI"/>
		<rdfs:comment xml:lang="en">JavaLibrary implementing the org.omg.CORBA.DynAnyPackage package for J2SE 5.0</rdfs:comment>
		<rdfs:comment xml:lang="OWLManchester">platform:comprisesInterfacePart some OrgOmgCORBADynAnyPackage</rdfs:comment>
	</owl:Class>
	<owl:Class rdf:about="&j2se-5_0;OrgOmgCORBAORBPackageAPI">
		<owl:equivalentClass rdf:resource="&j2se-1_4;OrgOmgCORBAORBPackageAPI"/>
		<rdfs:subClassOf rdf:resource="&java;JavaAPI"/>
		<rdfs:comment xml:lang="en">JavaLibrary implementing the org.omg.CORBA.ORBPackage package for J2SE 5.0</rdfs:comment>
		<rdfs:comment xml:lang="OWLManchester">platform:comprisesInterfacePart some OrgOmgCORBAORBPackage</rdfs:comment>
	</owl:Class>
	<owl:Class rdf:about="&j2se-5_0;OrgOmgCORBATypeCodePackageAPI">
		<owl:equivalentClass rdf:resource="&j2se-1_4;OrgOmgCORBATypeCodePackageAPI"/>
		<rdfs:subClassOf rdf:resource="&java;JavaAPI"/>
		<rdfs:comment xml:lang="en">JavaLibrary implementing the org.omg.CORBA.TypeCodePackage package for J2SE 5.0</rdfs:comment>
		<rdfs:comment xml:lang="OWLManchester">platform:comprisesInterfacePart some OrgOmgCORBATypeCodePackage</rdfs:comment>
	</owl:Class>
	<owl:Class rdf:about="&j2se-5_0;OrgOmgSendingContextAPI">
		<owl:equivalentClass rdf:resource="&j2se-1_4;OrgOmgSendingContextAPI"/>
		<rdfs:subClassOf rdf:resource="&java;JavaAPI"/>
		<rdfs:comment xml:lang="en">JavaLibrary implementing the org.omg.SendingContext package for J2SE 5.0</rdfs:comment>
		<rdfs:comment xml:lang="OWLManchester">platform:comprisesInterfacePart some OrgOmgSendingContext</rdfs:comment>
	</owl:Class>
	<owl:Class rdf:about="&j2se-5_0;OrgOmgCosNamingAPI">
		<rdfs:subClassOf rdf:resource="&j2se-1_4;OrgOmgCosNamingAPI"/>
		<rdfs:comment xml:lang="en">JavaLibrary implementing the org.omg.CosNaming package for J2SE 5.0</rdfs:comment>
		<rdfs:comment xml:lang="OWLManchester">platform:comprisesInterfacePart some OrgOmgCosNaming</rdfs:comment>
	</owl:Class>
	<owl:Class rdf:about="&j2se-5_0;OrgOmgCosNamingNamingContextExtPackageAPI">
		<owl:equivalentClass rdf:resource="&j2se-1_4;OrgOmgCosNamingNamingContextExtPackageAPI"/>
		<rdfs:subClassOf rdf:resource="&java;JavaAPI"/>
		<rdfs:comment xml:lang="en">JavaLibrary implementing the org.omg.CosNaming.NamingContextExtPackage package for J2SE 5.0</rdfs:comment>
		<rdfs:comment xml:lang="OWLManchester">platform:comprisesInterfacePart some OrgOmgCosNamingNamingContextExtPackage</rdfs:comment>
	</owl:Class>
	<owl:Class rdf:about="&j2se-5_0;OrgOmgCosNamingNamingContextPackageAPI">
		<owl:equivalentClass rdf:resource="&j2se-1_4;OrgOmgCosNamingNamingContextPackageAPI"/>
		<rdfs:subClassOf rdf:resource="&java;JavaAPI"/>
		<rdfs:comment xml:lang="en">JavaLibrary implementing the org.omg.CosNaming.NamingContextPackage package for J2SE 5.0</rdfs:comment>
		<rdfs:comment xml:lang="OWLManchester">platform:comprisesInterfacePart some OrgOmgCosNamingNamingContextPackage</rdfs:comment>
	</owl:Class>
	<owl:Class rdf:about="&j2se-5_0;OrgOmgPortableServerAPI">
		<rdfs:subClassOf rdf:resource="&j2se-1_4;OrgOmgPortableServerAPI"/>
		<rdfs:comment xml:lang="en">JavaLibrary implementing the org.omg.PortableServer package for J2SE 5.0</rdfs:comment>
		<rdfs:comment xml:lang="OWLManchester">platform:comprisesInterfacePart some OrgOmgPortableServer</rdfs:comment>
	</owl:Class>
	<owl:Class rdf:about="&j2se-5_0;OrgOmgPortableServerCurrentPackageAPI">
		<owl:equivalentClass rdf:resource="&j2se-1_4;OrgOmgPortableServerCurrentPackageAPI"/>
		<rdfs:subClassOf rdf:resource="&java;JavaAPI"/>
		<rdfs:comment xml:lang="en">JavaLibrary implementing the org.omg.PortableServer.CurrentPackage package for J2SE 5.0</rdfs:comment>
		<rdfs:comment xml:lang="OWLManchester">platform:comprisesInterfacePart some OrgOmgPortableServerCurrentPackage</rdfs:comment>
	</owl:Class>
	<owl:Class rdf:about="&j2se-5_0;OrgOmgPortableServerPOAManagerPackageAPI">
		<owl:equivalentClass rdf:resource="&j2se-1_4;OrgOmgPortableServerPOAManagerPackageAPI"/>
		<rdfs:subClassOf rdf:resource="&java;JavaAPI"/>
		<rdfs:comment xml:lang="en">JavaLibrary implementing the org.omg.PortableServer.POAManagerPackage package for J2SE 5.0</rdfs:comment>
		<rdfs:comment xml:lang="OWLManchester">platform:comprisesInterfacePart some OrgOmgPortableServerPOAManagerPackage</rdfs:comment>
	</owl:Class>
	<owl:Class rdf:about="&j2se-5_0;OrgOmgPortableServerPOAPackageAPI">
		<owl:equivalentClass rdf:resource="&j2se-1_4;OrgOmgPortableServerPOAPackageAPI"/>
		<rdfs:subClassOf rdf:resource="&java;JavaAPI"/>
		<rdfs:comment xml:lang="en">JavaLibrary implementing the org.omg.PortableServer.POAPackage package for J2SE 5.0</rdfs:comment>
		<rdfs:comment xml:lang="OWLManchester">platform:comprisesInterfacePart some OrgOmgPortableServerPOAPackage</rdfs:comment>
	</owl:Class>
	<owl:Class rdf:about="&j2se-5_0;OrgOmgPortableServerPortableAPI">
		<owl:equivalentClass rdf:resource="&j2se-1_4;OrgOmgPortableServerPortableAPI"/>
		<rdfs:subClassOf rdf:resource="&java;JavaAPI"/>
		<rdfs:comment xml:lang="en">JavaLibrary implementing the org.omg.PortableServer.portable package for J2SE 5.0</rdfs:comment>
		<rdfs:comment xml:lang="OWLManchester">platform:comprisesInterfacePart some OrgOmgPortableServerPortable</rdfs:comment>
	</owl:Class>
	<owl:Class rdf:about="&j2se-5_0;OrgOmgPortableServerServantLocatorPackageAPI">
		<owl:equivalentClass rdf:resource="&j2se-1_4;OrgOmgPortableServerServantLocatorPackageAPI"/>
		<rdfs:subClassOf rdf:resource="&java;JavaAPI"/>
		<rdfs:comment xml:lang="en">JavaLibrary implementing the org.omg.PortableServer.ServantLocatorPackage package for J2SE 5.0</rdfs:comment>
		<rdfs:comment xml:lang="OWLManchester">platform:comprisesInterfacePart some OrgOmgPortableServerServantLocatorPackage</rdfs:comment>
	</owl:Class>
	<owl:Class rdf:about="&j2se-5_0;OrgOmgDynamicAPI">
		<owl:equivalentClass rdf:resource="&j2se-1_4;OrgOmgDynamicAPI"/>
		<rdfs:subClassOf rdf:resource="&java;JavaAPI"/>
		<rdfs:comment xml:lang="en">JavaLibrary implementing the org.omg.Dynamic package for J2SE 5.0</rdfs:comment>
		<rdfs:comment xml:lang="OWLManchester">platform:comprisesInterfacePart some OrgOmgDynamic</rdfs:comment>
	</owl:Class>
	<owl:Class rdf:about="&j2se-5_0;OrgOmgDynamicAnyAPI">
		<rdfs:subClassOf rdf:resource="&j2se-1_4;OrgOmgDynamicAnyAPI"/>
		<rdfs:comment xml:lang="en">JavaLibrary implementing the org.omg.DynamicAny package for J2SE 5.0</rdfs:comment>
		<rdfs:comment xml:lang="OWLManchester">platform:comprisesInterfacePart some OrgOmgDynamicAny</rdfs:comment>
	</owl:Class>
	<owl:Class rdf:about="&j2se-5_0;OrgOmgDynamicAnyDynAnyFactoryPackageAPI">
		<owl:equivalentClass rdf:resource="&j2se-1_4;OrgOmgDynamicAnyDynAnyFactoryPackageAPI"/>
		<rdfs:subClassOf rdf:resource="&java;JavaAPI"/>
		<rdfs:comment xml:lang="en">JavaLibrary implementing the org.omg.DynamicAny.DynAnyFactoryPackage package for J2SE 5.0</rdfs:comment>
		<rdfs:comment xml:lang="OWLManchester">platform:comprisesInterfacePart some OrgOmgDynamicAnyDynAnyFactoryPackage</rdfs:comment>
	</owl:Class>
	<owl:Class rdf:about="&j2se-5_0;OrgOmgDynamicAnyDynAnyPackageAPI">
		<owl:equivalentClass rdf:resource="&j2se-1_4;OrgOmgDynamicAnyDynAnyPackageAPI"/>
		<rdfs:subClassOf rdf:resource="&java;JavaAPI"/>
		<rdfs:comment xml:lang="en">JavaLibrary implementing the org.omg.DynamicAny.DynAnyPackage package for J2SE 5.0</rdfs:comment>
		<rdfs:comment xml:lang="OWLManchester">platform:comprisesInterfacePart some OrgOmgDynamicAnyDynAnyPackage</rdfs:comment>
	</owl:Class>
	<owl:Class rdf:about="&j2se-5_0;OrgOmgIOPAPI">
		<rdfs:subClassOf rdf:resource="&j2se-1_4;OrgOmgIOPAPI"/>
		<rdfs:comment xml:lang="en">JavaLibrary implementing the org.omg.IOP package for J2SE 5.0</rdfs:comment>
		<rdfs:comment xml:lang="OWLManchester">platform:comprisesInterfacePart some OrgOmgIOP</rdfs:comment>
	</owl:Class>
	<owl:Class rdf:about="&j2se-5_0;OrgOmgIOPCodecFactoryPackageAPI">
		<owl:equivalentClass rdf:resource="&j2se-1_4;OrgOmgIOPCodecFactoryPackageAPI"/>
		<rdfs:subClassOf rdf:resource="&java;JavaAPI"/>
		<rdfs:comment xml:lang="en">JavaLibrary implementing the org.omg.IOP.CodecFactoryPackage package for J2SE 5.0</rdfs:comment>
		<rdfs:comment xml:lang="OWLManchester">platform:comprisesInterfacePart some OrgOmgIOPCodecFactoryPackage</rdfs:comment>
	</owl:Class>
	<owl:Class rdf:about="&j2se-5_0;OrgOmgIOPCodecPackageAPI">
		<owl:equivalentClass rdf:resource="&j2se-1_4;OrgOmgIOPCodecPackageAPI"/>
		<rdfs:subClassOf rdf:resource="&java;JavaAPI"/>
		<rdfs:comment xml:lang="en">JavaLibrary implementing the org.omg.IOP.CodecPackage package for J2SE 5.0</rdfs:comment>
		<rdfs:comment xml:lang="OWLManchester">platform:comprisesInterfacePart some OrgOmgIOPCodecPackage</rdfs:comment>
	</owl:Class>
	<owl:Class rdf:about="&j2se-5_0;OrgOmgMessagingAPI">
		<owl:equivalentClass rdf:resource="&j2se-1_4;OrgOmgMessagingAPI"/>
		<rdfs:subClassOf rdf:resource="&java;JavaAPI"/>
		<rdfs:comment xml:lang="en">JavaLibrary implementing the org.omg.Messaging package for J2SE 5.0</rdfs:comment>
		<rdfs:comment xml:lang="OWLManchester">platform:comprisesInterfacePart some OrgOmgMessaging</rdfs:comment>
	</owl:Class>
	<owl:Class rdf:about="&j2se-5_0;OrgOmgPortableInterceptorAPI">
		<rdfs:subClassOf rdf:resource="&j2se-1_4;OrgOmgPortableInterceptorAPI"/>
		<rdfs:comment xml:lang="en">JavaLibrary implementing the org.omg.PortableInterceptor package for J2SE 5.0</rdfs:comment>
		<rdfs:comment xml:lang="OWLManchester">platform:comprisesInterfacePart some OrgOmgPortableInterceptor</rdfs:comment>
	</owl:Class>
	<owl:Class rdf:about="&j2se-5_0;OrgOmgPortableInterceptorORBInitInfoPackageAPI">
		<owl:equivalentClass rdf:resource="&j2se-1_4;OrgOmgPortableInterceptorORBInitInfoPackageAPI"/>
		<rdfs:subClassOf rdf:resource="&java;JavaAPI"/>
		<rdfs:comment xml:lang="en">JavaLibrary implementing the org.omg.PortableInterceptor.ORBInitInfoPackage package for J2SE 5.0</rdfs:comment>
		<rdfs:comment xml:lang="OWLManchester">platform:comprisesInterfacePart some OrgOmgPortableInterceptorORBInitInfoPackage</rdfs:comment>
	</owl:Class>
	<owl:Class rdf:about="&j2se-5_0;OrgOmgStubJavaRmiAPI">
		<owl:equivalentClass rdf:resource="&j2se-1_4;OrgOmgStubJavaRmiAPI"/>
		<rdfs:subClassOf rdf:resource="&java;JavaAPI"/>
		<rdfs:comment xml:lang="en">JavaLibrary implementing the org.omg.stub.java.rmi package for J2SE 5.0</rdfs:comment>
		<rdfs:comment xml:lang="OWLManchester">platform:comprisesInterfacePart some OrgOmgStubJavaRmi</rdfs:comment>
	</owl:Class>
	<owl:Class rdf:about="&j2se-5_0;OrgOmgStubJavaxManagementRemoteRmiAPI">
		<rdfs:subClassOf rdf:resource="&java;JavaAPI"/>
		<rdfs:comment xml:lang="en">JavaLibrary implementing the org.omg.stub.javax.management.remote.rmi package for J2SE 5.0</rdfs:comment>
		<rdfs:comment xml:lang="OWLManchester">platform:comprisesInterfacePart some OrgOmgStubJavaxManagementRemoteRmi</rdfs:comment>
	</owl:Class>
	<owl:Class rdf:about="&j2se-5_0;OrgXmlSaxAPI">
		<owl:equivalentClass rdf:resource="&j2se-1_4;OrgXmlSaxAPI"/>
		<rdfs:subClassOf rdf:resource="&java;JavaAPI"/>
		<rdfs:comment xml:lang="en">JavaLibrary implementing the org.xml.sax package for J2SE 5.0</rdfs:comment>
		<rdfs:comment xml:lang="OWLManchester">platform:comprisesInterfacePart some OrgXmlSax</rdfs:comment>
	</owl:Class>
	<owl:Class rdf:about="&j2se-5_0;OrgXmlSaxExtAPI">
		<rdfs:subClassOf rdf:resource="&j2se-1_4;OrgXmlSaxExtAPI"/>
		<rdfs:comment xml:lang="en">JavaLibrary implementing the org.xml.sax.ext package for J2SE 5.0</rdfs:comment>
		<rdfs:comment xml:lang="OWLManchester">platform:comprisesInterfacePart some OrgXmlSaxExt</rdfs:comment>
	</owl:Class>
	<owl:Class rdf:about="&j2se-5_0;OrgXmlSaxHelpersAPI">
		<rdfs:subClassOf rdf:resource="&j2se-1_4;OrgXmlSaxHelpersAPI"/>
		<rdfs:comment xml:lang="en">JavaLibrary implementing the org.xml.sax.helpers package for J2SE 5.0</rdfs:comment>
		<rdfs:comment xml:lang="OWLManchester">platform:comprisesInterfacePart some OrgXmlSaxHelpers</rdfs:comment>
	</owl:Class>
	<owl:Class rdf:about="&j2se-5_0;OrgIetfJgssAPI">
		<owl:equivalentClass rdf:resource="&j2se-1_4;OrgIetfJgssAPI"/>
		<rdfs:subClassOf rdf:resource="&java;JavaAPI"/>
		<rdfs:comment xml:lang="en">JavaLibrary implementing the org.ietf.jgss package for J2SE 5.0</rdfs:comment>
		<rdfs:comment xml:lang="OWLManchester">platform:comprisesInterfacePart some OrgIetfJgss</rdfs:comment>
	</owl:Class>
	<j2se-5_0:JavaxCrypto rdf:about="&j2se-5_0;theJavaxCryptoPart">
	</j2se-5_0:JavaxCrypto>
	<j2se-5_0:JavaxCryptoInterfaces rdf:about="&j2se-5_0;theJavaxCryptoInterfacesPart">
	</j2se-5_0:JavaxCryptoInterfaces>
	<j2se-5_0:JavaxCryptoSpec rdf:about="&j2se-5_0;theJavaxCryptoSpecPart">
	</j2se-5_0:JavaxCryptoSpec>
	<j2se-5_0:JavaxNet rdf:about="&j2se-5_0;theJavaxNetPart">
	</j2se-5_0:JavaxNet>
	<j2se-5_0:JavaxNetSsl rdf:about="&j2se-5_0;theJavaxNetSslPart">
	</j2se-5_0:JavaxNetSsl>
	<j2se-5_0:JavaxSecurityCert rdf:about="&j2se-5_0;theJavaxSecurityCertPart">
	</j2se-5_0:JavaxSecurityCert>
	<j2se-5_0:JavaxSecurityAuth rdf:about="&j2se-5_0;theJavaxSecurityAuthPart">
	</j2se-5_0:JavaxSecurityAuth>
	<j2se-5_0:JavaxSecurityAuthCallback rdf:about="&j2se-5_0;theJavaxSecurityAuthCallbackPart">
	</j2se-5_0:JavaxSecurityAuthCallback>
	<j2se-5_0:JavaxSecurityAuthX500 rdf:about="&j2se-5_0;theJavaxSecurityAuthX500Part">
	</j2se-5_0:JavaxSecurityAuthX500>
	<j2se-5_0:JavaxSecurityAuthKerberos rdf:about="&j2se-5_0;theJavaxSecurityAuthKerberosPart">
	</j2se-5_0:JavaxSecurityAuthKerberos>
	<j2se-5_0:JavaxSecurityAuthLogin rdf:about="&j2se-5_0;theJavaxSecurityAuthLoginPart">
	</j2se-5_0:JavaxSecurityAuthLogin>
	<j2se-5_0:JavaxSecurityAuthSpi rdf:about="&j2se-5_0;theJavaxSecurityAuthSpiPart">
	</j2se-5_0:JavaxSecurityAuthSpi>
	<j2se-5_0:JavaxSecuritySasl rdf:about="&j2se-5_0;theJavaxSecuritySaslPart">
	</j2se-5_0:JavaxSecuritySasl>
	<j2se-5_0:JavaxAccessibility rdf:about="&j2se-5_0;theJavaxAccessibilityPart">
	</j2se-5_0:JavaxAccessibility>
	<j2se-5_0:JavaxSwing rdf:about="&j2se-5_0;theJavaxSwingPart">
	</j2se-5_0:JavaxSwing>
	<j2se-5_0:JavaxSwingText rdf:about="&j2se-5_0;theJavaxSwingTextPart">
	</j2se-5_0:JavaxSwingText>
	<j2se-5_0:JavaxSwingTextHtml rdf:about="&j2se-5_0;theJavaxSwingTextHtmlPart">
	</j2se-5_0:JavaxSwingTextHtml>
	<j2se-5_0:JavaxSwingTextHtmlParser rdf:about="&j2se-5_0;theJavaxSwingTextHtmlParserPart">
	</j2se-5_0:JavaxSwingTextHtmlParser>
	<j2se-5_0:JavaxSwingTextRtf rdf:about="&j2se-5_0;theJavaxSwingTextRtfPart">
	</j2se-5_0:JavaxSwingTextRtf>
	<j2se-5_0:JavaxSwingEvent rdf:about="&j2se-5_0;theJavaxSwingEventPart">
	</j2se-5_0:JavaxSwingEvent>
	<j2se-5_0:JavaxSwingColorchooser rdf:about="&j2se-5_0;theJavaxSwingColorchooserPart">
	</j2se-5_0:JavaxSwingColorchooser>
	<j2se-5_0:JavaxSwingPlaf rdf:about="&j2se-5_0;theJavaxSwingPlafPart">
	</j2se-5_0:JavaxSwingPlaf>
	<j2se-5_0:JavaxSwingPlafBasic rdf:about="&j2se-5_0;theJavaxSwingPlafBasicPart">
	</j2se-5_0:JavaxSwingPlafBasic>
	<j2se-5_0:JavaxSwingPlafMetal rdf:about="&j2se-5_0;theJavaxSwingPlafMetalPart">
	</j2se-5_0:JavaxSwingPlafMetal>
	<j2se-5_0:JavaxSwingPlafMulti rdf:about="&j2se-5_0;theJavaxSwingPlafMultiPart">
	</j2se-5_0:JavaxSwingPlafMulti>
	<j2se-5_0:JavaxSwingPlafSynth rdf:about="&j2se-5_0;theJavaxSwingPlafSynthPart">
	</j2se-5_0:JavaxSwingPlafSynth>
	<j2se-5_0:JavaxSwingTree rdf:about="&j2se-5_0;theJavaxSwingTreePart">
	</j2se-5_0:JavaxSwingTree>
	<j2se-5_0:JavaxSwingBorder rdf:about="&j2se-5_0;theJavaxSwingBorderPart">
	</j2se-5_0:JavaxSwingBorder>
	<j2se-5_0:JavaxSwingFilechooser rdf:about="&j2se-5_0;theJavaxSwingFilechooserPart">
	</j2se-5_0:JavaxSwingFilechooser>
	<j2se-5_0:JavaxSwingTable rdf:about="&j2se-5_0;theJavaxSwingTablePart">
	</j2se-5_0:JavaxSwingTable>
	<j2se-5_0:JavaxSwingUndo rdf:about="&j2se-5_0;theJavaxSwingUndoPart">
	</j2se-5_0:JavaxSwingUndo>
	<j2se-5_0:JavaxManagement rdf:about="&j2se-5_0;theJavaxManagementPart">
	</j2se-5_0:JavaxManagement>
	<j2se-5_0:JavaxManagementOpenmbean rdf:about="&j2se-5_0;theJavaxManagementOpenmbeanPart">
	</j2se-5_0:JavaxManagementOpenmbean>
	<j2se-5_0:JavaxManagementLoading rdf:about="&j2se-5_0;theJavaxManagementLoadingPart">
	</j2se-5_0:JavaxManagementLoading>
	<j2se-5_0:JavaxManagementModelmbean rdf:about="&j2se-5_0;theJavaxManagementModelmbeanPart">
	</j2se-5_0:JavaxManagementModelmbean>
	<j2se-5_0:JavaxManagementMonitor rdf:about="&j2se-5_0;theJavaxManagementMonitorPart">
	</j2se-5_0:JavaxManagementMonitor>
	<j2se-5_0:JavaxManagementRelation rdf:about="&j2se-5_0;theJavaxManagementRelationPart">
	</j2se-5_0:JavaxManagementRelation>
	<j2se-5_0:JavaxManagementRemote rdf:about="&j2se-5_0;theJavaxManagementRemotePart">
	</j2se-5_0:JavaxManagementRemote>
	<j2se-5_0:JavaxManagementRemoteRmi rdf:about="&j2se-5_0;theJavaxManagementRemoteRmiPart">
	</j2se-5_0:JavaxManagementRemoteRmi>
	<j2se-5_0:JavaxManagementTimer rdf:about="&j2se-5_0;theJavaxManagementTimerPart">
	</j2se-5_0:JavaxManagementTimer>
	<j2se-5_0:JavaxActivity rdf:about="&j2se-5_0;theJavaxActivityPart">
	</j2se-5_0:JavaxActivity>
	<j2se-5_0:JavaxImageio rdf:about="&j2se-5_0;theJavaxImageioPart">
	</j2se-5_0:JavaxImageio>
	<j2se-5_0:JavaxImageioMetadata rdf:about="&j2se-5_0;theJavaxImageioMetadataPart">
	</j2se-5_0:JavaxImageioMetadata>
	<j2se-5_0:JavaxImageioEvent rdf:about="&j2se-5_0;theJavaxImageioEventPart">
	</j2se-5_0:JavaxImageioEvent>
	<j2se-5_0:JavaxImageioPluginsBmp rdf:about="&j2se-5_0;theJavaxImageioPluginsBmpPart">
	</j2se-5_0:JavaxImageioPluginsBmp>
	<j2se-5_0:JavaxImageioPluginsJpeg rdf:about="&j2se-5_0;theJavaxImageioPluginsJpegPart">
	</j2se-5_0:JavaxImageioPluginsJpeg>
	<j2se-5_0:JavaxImageioStream rdf:about="&j2se-5_0;theJavaxImageioStreamPart">
	</j2se-5_0:JavaxImageioStream>
	<j2se-5_0:JavaxImageioSpi rdf:about="&j2se-5_0;theJavaxImageioSpiPart">
	</j2se-5_0:JavaxImageioSpi>
	<j2se-5_0:JavaxNaming rdf:about="&j2se-5_0;theJavaxNamingPart">
	</j2se-5_0:JavaxNaming>
	<j2se-5_0:JavaxNamingDirectory rdf:about="&j2se-5_0;theJavaxNamingDirectoryPart">
	</j2se-5_0:JavaxNamingDirectory>
	<j2se-5_0:JavaxNamingEvent rdf:about="&j2se-5_0;theJavaxNamingEventPart">
	</j2se-5_0:JavaxNamingEvent>
	<j2se-5_0:JavaxNamingLdap rdf:about="&j2se-5_0;theJavaxNamingLdapPart">
	</j2se-5_0:JavaxNamingLdap>
	<j2se-5_0:JavaxNamingSpi rdf:about="&j2se-5_0;theJavaxNamingSpiPart">
	</j2se-5_0:JavaxNamingSpi>
	<j2se-5_0:JavaxPrint rdf:about="&j2se-5_0;theJavaxPrintPart">
	</j2se-5_0:JavaxPrint>
	<j2se-5_0:JavaxPrintAttribute rdf:about="&j2se-5_0;theJavaxPrintAttributePart">
	</j2se-5_0:JavaxPrintAttribute>
	<j2se-5_0:JavaxPrintAttributeStandard rdf:about="&j2se-5_0;theJavaxPrintAttributeStandardPart">
	</j2se-5_0:JavaxPrintAttributeStandard>
	<j2se-5_0:JavaxPrintEvent rdf:about="&j2se-5_0;theJavaxPrintEventPart">
	</j2se-5_0:JavaxPrintEvent>
	<j2se-5_0:JavaxRmi rdf:about="&j2se-5_0;theJavaxRmiPart">
	</j2se-5_0:JavaxRmi>
	<j2se-5_0:JavaxRmiCORBA rdf:about="&j2se-5_0;theJavaxRmiCORBAPart">
	</j2se-5_0:JavaxRmiCORBA>
	<j2se-5_0:JavaxRmiSsl rdf:about="&j2se-5_0;theJavaxRmiSslPart">
	</j2se-5_0:JavaxRmiSsl>
	<j2se-5_0:JavaxSoundMidi rdf:about="&j2se-5_0;theJavaxSoundMidiPart">
	</j2se-5_0:JavaxSoundMidi>
	<j2se-5_0:JavaxSoundMidiSpi rdf:about="&j2se-5_0;theJavaxSoundMidiSpiPart">
	</j2se-5_0:JavaxSoundMidiSpi>
	<j2se-5_0:JavaxSoundSampled rdf:about="&j2se-5_0;theJavaxSoundSampledPart">
	</j2se-5_0:JavaxSoundSampled>
	<j2se-5_0:JavaxSoundSampledSpi rdf:about="&j2se-5_0;theJavaxSoundSampledSpiPart">
	</j2se-5_0:JavaxSoundSampledSpi>
	<j2se-5_0:JavaxSql rdf:about="&j2se-5_0;theJavaxSqlPart">
	</j2se-5_0:JavaxSql>
	<j2se-5_0:JavaxSqlRowset rdf:about="&j2se-5_0;theJavaxSqlRowsetPart">
	</j2se-5_0:JavaxSqlRowset>
	<j2se-5_0:JavaxSqlRowsetSpi rdf:about="&j2se-5_0;theJavaxSqlRowsetSpiPart">
	</j2se-5_0:JavaxSqlRowsetSpi>
	<j2se-5_0:JavaxSqlRowsetSerial rdf:about="&j2se-5_0;theJavaxSqlRowsetSerialPart">
	</j2se-5_0:JavaxSqlRowsetSerial>
	<j2se-5_0:JavaxTransaction rdf:about="&j2se-5_0;theJavaxTransactionPart">
	</j2se-5_0:JavaxTransaction>
	<j2se-5_0:JavaxTransactionXa rdf:about="&j2se-5_0;theJavaxTransactionXaPart">
	</j2se-5_0:JavaxTransactionXa>
	<j2se-5_0:JavaxXml rdf:about="&j2se-5_0;theJavaxXmlPart">
	</j2se-5_0:JavaxXml>
	<j2se-5_0:JavaxXmlDatatype rdf:about="&j2se-5_0;theJavaxXmlDatatypePart">
	</j2se-5_0:JavaxXmlDatatype>
	<j2se-5_0:JavaxXmlNamespace rdf:about="&j2se-5_0;theJavaxXmlNamespacePart">
	</j2se-5_0:JavaxXmlNamespace>
	<j2se-5_0:JavaxXmlTransform rdf:about="&j2se-5_0;theJavaxXmlTransformPart">
	</j2se-5_0:JavaxXmlTransform>
	<j2se-5_0:JavaxXmlTransformDom rdf:about="&j2se-5_0;theJavaxXmlTransformDomPart">
	</j2se-5_0:JavaxXmlTransformDom>
	<j2se-5_0:JavaxXmlTransformSax rdf:about="&j2se-5_0;theJavaxXmlTransformSaxPart">
	</j2se-5_0:JavaxXmlTransformSax>
	<j2se-5_0:JavaxXmlTransformStream rdf:about="&j2se-5_0;theJavaxXmlTransformStreamPart">
	</j2se-5_0:JavaxXmlTransformStream>
	<j2se-5_0:JavaxXmlValidation rdf:about="&j2se-5_0;theJavaxXmlValidationPart">
	</j2se-5_0:JavaxXmlValidation>
	<j2se-5_0:JavaxXmlXpath rdf:about="&j2se-5_0;theJavaxXmlXpathPart">
	</j2se-5_0:JavaxXmlXpath>
	<j2se-5_0:JavaxXmlParsers rdf:about="&j2se-5_0;theJavaxXmlParsersPart">
	</j2se-5_0:JavaxXmlParsers>
	<j2se-5_0:JavaLang rdf:about="&j2se-5_0;theJavaLangPart">
	</j2se-5_0:JavaLang>
	<j2se-5_0:JavaLangReflect rdf:about="&j2se-5_0;theJavaLangReflectPart">
	</j2se-5_0:JavaLangReflect>
	<j2se-5_0:JavaLangAnnotation rdf:about="&j2se-5_0;theJavaLangAnnotationPart">
	</j2se-5_0:JavaLangAnnotation>
	<j2se-5_0:JavaLangInstrument rdf:about="&j2se-5_0;theJavaLangInstrumentPart">
	</j2se-5_0:JavaLangInstrument>
	<j2se-5_0:JavaLangManagement rdf:about="&j2se-5_0;theJavaLangManagementPart">
	</j2se-5_0:JavaLangManagement>
	<j2se-5_0:JavaLangRef rdf:about="&j2se-5_0;theJavaLangRefPart">
	</j2se-5_0:JavaLangRef>
	<j2se-5_0:JavaSecurity rdf:about="&j2se-5_0;theJavaSecurityPart">
	</j2se-5_0:JavaSecurity>
	<j2se-5_0:JavaSecuritySpec rdf:about="&j2se-5_0;theJavaSecuritySpecPart">
	</j2se-5_0:JavaSecuritySpec>
	<j2se-5_0:JavaSecurityCert rdf:about="&j2se-5_0;theJavaSecurityCertPart">
	</j2se-5_0:JavaSecurityCert>
	<j2se-5_0:JavaSecurityAcl rdf:about="&j2se-5_0;theJavaSecurityAclPart">
	</j2se-5_0:JavaSecurityAcl>
	<j2se-5_0:JavaSecurityInterfaces rdf:about="&j2se-5_0;theJavaSecurityInterfacesPart">
	</j2se-5_0:JavaSecurityInterfaces>
	<j2se-5_0:JavaMath rdf:about="&j2se-5_0;theJavaMathPart">
	</j2se-5_0:JavaMath>
	<j2se-5_0:JavaNio rdf:about="&j2se-5_0;theJavaNioPart">
	</j2se-5_0:JavaNio>
	<j2se-5_0:JavaNioChannels rdf:about="&j2se-5_0;theJavaNioChannelsPart">
	</j2se-5_0:JavaNioChannels>
	<j2se-5_0:JavaNioChannelsSpi rdf:about="&j2se-5_0;theJavaNioChannelsSpiPart">
	</j2se-5_0:JavaNioChannelsSpi>
	<j2se-5_0:JavaNioCharset rdf:about="&j2se-5_0;theJavaNioCharsetPart">
	</j2se-5_0:JavaNioCharset>
	<j2se-5_0:JavaNioCharsetSpi rdf:about="&j2se-5_0;theJavaNioCharsetSpiPart">
	</j2se-5_0:JavaNioCharsetSpi>
	<j2se-5_0:JavaIo rdf:about="&j2se-5_0;theJavaIoPart">
	</j2se-5_0:JavaIo>
	<j2se-5_0:JavaNet rdf:about="&j2se-5_0;theJavaNetPart">
	</j2se-5_0:JavaNet>
	<j2se-5_0:JavaUtil rdf:about="&j2se-5_0;theJavaUtilPart">
	</j2se-5_0:JavaUtil>
	<j2se-5_0:JavaUtilRegex rdf:about="&j2se-5_0;theJavaUtilRegexPart">
	</j2se-5_0:JavaUtilRegex>
	<j2se-5_0:JavaUtilConcurrent rdf:about="&j2se-5_0;theJavaUtilConcurrentPart">
	</j2se-5_0:JavaUtilConcurrent>
	<j2se-5_0:JavaUtilConcurrentAtomic rdf:about="&j2se-5_0;theJavaUtilConcurrentAtomicPart">
	</j2se-5_0:JavaUtilConcurrentAtomic>
	<j2se-5_0:JavaUtilConcurrentLocks rdf:about="&j2se-5_0;theJavaUtilConcurrentLocksPart">
	</j2se-5_0:JavaUtilConcurrentLocks>
	<j2se-5_0:JavaUtilJar rdf:about="&j2se-5_0;theJavaUtilJarPart">
	</j2se-5_0:JavaUtilJar>
	<j2se-5_0:JavaUtilZip rdf:about="&j2se-5_0;theJavaUtilZipPart">
	</j2se-5_0:JavaUtilZip>
	<j2se-5_0:JavaUtilLogging rdf:about="&j2se-5_0;theJavaUtilLoggingPart">
	</j2se-5_0:JavaUtilLogging>
	<j2se-5_0:JavaUtilPrefs rdf:about="&j2se-5_0;theJavaUtilPrefsPart">
	</j2se-5_0:JavaUtilPrefs>
	<j2se-5_0:JavaApplet rdf:about="&j2se-5_0;theJavaAppletPart">
	</j2se-5_0:JavaApplet>
	<j2se-5_0:JavaAwt rdf:about="&j2se-5_0;theJavaAwtPart">
	</j2se-5_0:JavaAwt>
	<j2se-5_0:JavaAwtEvent rdf:about="&j2se-5_0;theJavaAwtEventPart">
	</j2se-5_0:JavaAwtEvent>
	<j2se-5_0:JavaAwtImage rdf:about="&j2se-5_0;theJavaAwtImagePart">
	</j2se-5_0:JavaAwtImage>
	<j2se-5_0:JavaAwtImageRenderable rdf:about="&j2se-5_0;theJavaAwtImageRenderablePart">
	</j2se-5_0:JavaAwtImageRenderable>
	<j2se-5_0:JavaAwtGeom rdf:about="&j2se-5_0;theJavaAwtGeomPart">
	</j2se-5_0:JavaAwtGeom>
	<j2se-5_0:JavaAwtIm rdf:about="&j2se-5_0;theJavaAwtImPart">
	</j2se-5_0:JavaAwtIm>
	<j2se-5_0:JavaAwtImSpi rdf:about="&j2se-5_0;theJavaAwtImSpiPart">
	</j2se-5_0:JavaAwtImSpi>
	<j2se-5_0:JavaAwtColor rdf:about="&j2se-5_0;theJavaAwtColorPart">
	</j2se-5_0:JavaAwtColor>
	<j2se-5_0:JavaAwtDatatransfer rdf:about="&j2se-5_0;theJavaAwtDatatransferPart">
	</j2se-5_0:JavaAwtDatatransfer>
	<j2se-5_0:JavaAwtDnd rdf:about="&j2se-5_0;theJavaAwtDndPart">
	</j2se-5_0:JavaAwtDnd>
	<j2se-5_0:JavaAwtFont rdf:about="&j2se-5_0;theJavaAwtFontPart">
	</j2se-5_0:JavaAwtFont>
	<j2se-5_0:JavaAwtPrint rdf:about="&j2se-5_0;theJavaAwtPrintPart">
	</j2se-5_0:JavaAwtPrint>
	<j2se-5_0:JavaText rdf:about="&j2se-5_0;theJavaTextPart">
	</j2se-5_0:JavaText>
	<j2se-5_0:JavaBeans rdf:about="&j2se-5_0;theJavaBeansPart">
	</j2se-5_0:JavaBeans>
	<j2se-5_0:JavaBeansBeancontext rdf:about="&j2se-5_0;theJavaBeansBeancontextPart">
	</j2se-5_0:JavaBeansBeancontext>
	<j2se-5_0:JavaRmi rdf:about="&j2se-5_0;theJavaRmiPart">
	</j2se-5_0:JavaRmi>
	<j2se-5_0:JavaRmiActivation rdf:about="&j2se-5_0;theJavaRmiActivationPart">
	</j2se-5_0:JavaRmiActivation>
	<j2se-5_0:JavaRmiServer rdf:about="&j2se-5_0;theJavaRmiServerPart">
	</j2se-5_0:JavaRmiServer>
	<j2se-5_0:JavaRmiDgc rdf:about="&j2se-5_0;theJavaRmiDgcPart">
	</j2se-5_0:JavaRmiDgc>
	<j2se-5_0:JavaRmiRegistry rdf:about="&j2se-5_0;theJavaRmiRegistryPart">
	</j2se-5_0:JavaRmiRegistry>
	<j2se-5_0:JavaSql rdf:about="&j2se-5_0;theJavaSqlPart">
	</j2se-5_0:JavaSql>
	<j2se-5_0:OrgW3cDom rdf:about="&j2se-5_0;theOrgW3cDomPart">
	</j2se-5_0:OrgW3cDom>
	<j2se-5_0:OrgW3cDomLs rdf:about="&j2se-5_0;theOrgW3cDomLsPart">
	</j2se-5_0:OrgW3cDomLs>
	<j2se-5_0:OrgW3cDomBootstrap rdf:about="&j2se-5_0;theOrgW3cDomBootstrapPart">
	</j2se-5_0:OrgW3cDomBootstrap>
	<j2se-5_0:OrgW3cDomCss rdf:about="&j2se-5_0;theOrgW3cDomCssPart">
	</j2se-5_0:OrgW3cDomCss>
	<j2se-5_0:OrgW3cDomStylesheets rdf:about="&j2se-5_0;theOrgW3cDomStylesheetsPart">
	</j2se-5_0:OrgW3cDomStylesheets>
	<j2se-5_0:OrgW3cDomViews rdf:about="&j2se-5_0;theOrgW3cDomViewsPart">
	</j2se-5_0:OrgW3cDomViews>
	<j2se-5_0:OrgW3cDomEvents rdf:about="&j2se-5_0;theOrgW3cDomEventsPart">
	</j2se-5_0:OrgW3cDomEvents>
	<j2se-5_0:OrgW3cDomHtml rdf:about="&j2se-5_0;theOrgW3cDomHtmlPart">
	</j2se-5_0:OrgW3cDomHtml>
	<j2se-5_0:OrgW3cDomTraversal rdf:about="&j2se-5_0;theOrgW3cDomTraversalPart">
	</j2se-5_0:OrgW3cDomTraversal>
	<j2se-5_0:OrgW3cDomRanges rdf:about="&j2se-5_0;theOrgW3cDomRangesPart">
	</j2se-5_0:OrgW3cDomRanges>
	<j2se-5_0:OrgOmgCORBA_2_3 rdf:about="&j2se-5_0;theOrgOmgCORBA_2_3Part">
	</j2se-5_0:OrgOmgCORBA_2_3>
	<j2se-5_0:OrgOmgCORBA_2_3Portable rdf:about="&j2se-5_0;theOrgOmgCORBA_2_3PortablePart">
	</j2se-5_0:OrgOmgCORBA_2_3Portable>
	<j2se-5_0:OrgOmgCORBA rdf:about="&j2se-5_0;theOrgOmgCORBAPart">
	</j2se-5_0:OrgOmgCORBA>
	<j2se-5_0:OrgOmgCORBAPortable rdf:about="&j2se-5_0;theOrgOmgCORBAPortablePart">
	</j2se-5_0:OrgOmgCORBAPortable>
	<j2se-5_0:OrgOmgCORBADynAnyPackage rdf:about="&j2se-5_0;theOrgOmgCORBADynAnyPackagePart">
	</j2se-5_0:OrgOmgCORBADynAnyPackage>
	<j2se-5_0:OrgOmgCORBAORBPackage rdf:about="&j2se-5_0;theOrgOmgCORBAORBPackagePart">
	</j2se-5_0:OrgOmgCORBAORBPackage>
	<j2se-5_0:OrgOmgCORBATypeCodePackage rdf:about="&j2se-5_0;theOrgOmgCORBATypeCodePackagePart">
	</j2se-5_0:OrgOmgCORBATypeCodePackage>
	<j2se-5_0:OrgOmgSendingContext rdf:about="&j2se-5_0;theOrgOmgSendingContextPart">
	</j2se-5_0:OrgOmgSendingContext>
	<j2se-5_0:OrgOmgCosNaming rdf:about="&j2se-5_0;theOrgOmgCosNamingPart">
	</j2se-5_0:OrgOmgCosNaming>
	<j2se-5_0:OrgOmgCosNamingNamingContextExtPackage rdf:about="&j2se-5_0;theOrgOmgCosNamingNamingContextExtPackagePart">
	</j2se-5_0:OrgOmgCosNamingNamingContextExtPackage>
	<j2se-5_0:OrgOmgCosNamingNamingContextPackage rdf:about="&j2se-5_0;theOrgOmgCosNamingNamingContextPackagePart">
	</j2se-5_0:OrgOmgCosNamingNamingContextPackage>
	<j2se-5_0:OrgOmgPortableServer rdf:about="&j2se-5_0;theOrgOmgPortableServerPart">
	</j2se-5_0:OrgOmgPortableServer>
	<j2se-5_0:OrgOmgPortableServerCurrentPackage rdf:about="&j2se-5_0;theOrgOmgPortableServerCurrentPackagePart">
	</j2se-5_0:OrgOmgPortableServerCurrentPackage>
	<j2se-5_0:OrgOmgPortableServerPOAManagerPackage rdf:about="&j2se-5_0;theOrgOmgPortableServerPOAManagerPackagePart">
	</j2se-5_0:OrgOmgPortableServerPOAManagerPackage>
	<j2se-5_0:OrgOmgPortableServerPOAPackage rdf:about="&j2se-5_0;theOrgOmgPortableServerPOAPackagePart">
	</j2se-5_0:OrgOmgPortableServerPOAPackage>
	<j2se-5_0:OrgOmgPortableServerPortable rdf:about="&j2se-5_0;theOrgOmgPortableServerPortablePart">
	</j2se-5_0:OrgOmgPortableServerPortable>
	<j2se-5_0:OrgOmgPortableServerServantLocatorPackage rdf:about="&j2se-5_0;theOrgOmgPortableServerServantLocatorPackagePart">
	</j2se-5_0:OrgOmgPortableServerServantLocatorPackage>
	<j2se-5_0:OrgOmgDynamic rdf:about="&j2se-5_0;theOrgOmgDynamicPart">
	</j2se-5_0:OrgOmgDynamic>
	<j2se-5_0:OrgOmgDynamicAny rdf:about="&j2se-5_0;theOrgOmgDynamicAnyPart">
	</j2se-5_0:OrgOmgDynamicAny>
	<j2se-5_0:OrgOmgDynamicAnyDynAnyFactoryPackage rdf:about="&j2se-5_0;theOrgOmgDynamicAnyDynAnyFactoryPackagePart">
	</j2se-5_0:OrgOmgDynamicAnyDynAnyFactoryPackage>
	<j2se-5_0:OrgOmgDynamicAnyDynAnyPackage rdf:about="&j2se-5_0;theOrgOmgDynamicAnyDynAnyPackagePart">
	</j2se-5_0:OrgOmgDynamicAnyDynAnyPackage>
	<j2se-5_0:OrgOmgIOP rdf:about="&j2se-5_0;theOrgOmgIOPPart">
	</j2se-5_0:OrgOmgIOP>
	<j2se-5_0:OrgOmgIOPCodecFactoryPackage rdf:about="&j2se-5_0;theOrgOmgIOPCodecFactoryPackagePart">
	</j2se-5_0:OrgOmgIOPCodecFactoryPackage>
	<j2se-5_0:OrgOmgIOPCodecPackage rdf:about="&j2se-5_0;theOrgOmgIOPCodecPackagePart">
	</j2se-5_0:OrgOmgIOPCodecPackage>
	<j2se-5_0:OrgOmgMessaging rdf:about="&j2se-5_0;theOrgOmgMessagingPart">
	</j2se-5_0:OrgOmgMessaging>
	<j2se-5_0:OrgOmgPortableInterceptor rdf:about="&j2se-5_0;theOrgOmgPortableInterceptorPart">
	</j2se-5_0:OrgOmgPortableInterceptor>
	<j2se-5_0:OrgOmgPortableInterceptorORBInitInfoPackage rdf:about="&j2se-5_0;theOrgOmgPortableInterceptorORBInitInfoPackagePart">
	</j2se-5_0:OrgOmgPortableInterceptorORBInitInfoPackage>
	<j2se-5_0:OrgOmgStubJavaRmi rdf:about="&j2se-5_0;theOrgOmgStubJavaRmiPart">
	</j2se-5_0:OrgOmgStubJavaRmi>
	<j2se-5_0:OrgOmgStubJavaxManagementRemoteRmi rdf:about="&j2se-5_0;theOrgOmgStubJavaxManagementRemoteRmiPart">
	</j2se-5_0:OrgOmgStubJavaxManagementRemoteRmi>
	<j2se-5_0:OrgXmlSax rdf:about="&j2se-5_0;theOrgXmlSaxPart">
	</j2se-5_0:OrgXmlSax>
	<j2se-5_0:OrgXmlSaxExt rdf:about="&j2se-5_0;theOrgXmlSaxExtPart">
	</j2se-5_0:OrgXmlSaxExt>
	<j2se-5_0:OrgXmlSaxHelpers rdf:about="&j2se-5_0;theOrgXmlSaxHelpersPart">
	</j2se-5_0:OrgXmlSaxHelpers>
	<j2se-5_0:OrgIetfJgss rdf:about="&j2se-5_0;theOrgIetfJgssPart">
	</j2se-5_0:OrgIetfJgss>
	<owl:Class rdf:about="&j2se-5_0;JavaxCryptoClassLibrary">
		<rdfs:subClassOf rdf:resource="&j2se-1_4;JavaxCryptoClassLibrary"/>
		<rdfs:comment xml:lang="en">JavaLibrary implementing the javax.crypto package for J2SE 5.0</rdfs:comment>
		<rdfs:comment xml:lang="OWLManchester">platform:implementsInterface some JavaxCryptoAPI</rdfs:comment>
	</owl:Class>
	<owl:Class rdf:about="&j2se-5_0;JavaxCryptoInterfacesClassLibrary">
		<owl:equivalentClass rdf:resource="&j2se-1_4;JavaxCryptoInterfacesClassLibrary"/>
		<rdfs:subClassOf rdf:resource="&java;JavaClassLibrary"/>
		<rdfs:comment xml:lang="en">JavaLibrary implementing the javax.crypto.interfaces package for J2SE 5.0</rdfs:comment>
		<rdfs:comment xml:lang="OWLManchester">platform:implementsInterface some JavaxCryptoInterfacesAPI</rdfs:comment>
	</owl:Class>
	<owl:Class rdf:about="&j2se-5_0;JavaxCryptoSpecClassLibrary">
		<rdfs:subClassOf rdf:resource="&j2se-1_4;JavaxCryptoSpecClassLibrary"/>
		<rdfs:comment xml:lang="en">JavaLibrary implementing the javax.crypto.spec package for J2SE 5.0</rdfs:comment>
		<rdfs:comment xml:lang="OWLManchester">platform:implementsInterface some JavaxCryptoSpecAPI</rdfs:comment>
	</owl:Class>
	<owl:Class rdf:about="&j2se-5_0;JavaxNetClassLibrary">
		<owl:equivalentClass rdf:resource="&j2se-1_4;JavaxNetClassLibrary"/>
		<rdfs:subClassOf rdf:resource="&java;JavaClassLibrary"/>
		<rdfs:comment xml:lang="en">JavaLibrary implementing the javax.net package for J2SE 5.0</rdfs:comment>
		<rdfs:comment xml:lang="OWLManchester">platform:implementsInterface some JavaxNetAPI</rdfs:comment>
	</owl:Class>
	<owl:Class rdf:about="&j2se-5_0;JavaxNetSslClassLibrary">
		<rdfs:subClassOf rdf:resource="&j2se-1_4;JavaxNetSslClassLibrary"/>
		<rdfs:comment xml:lang="en">JavaLibrary implementing the javax.net.ssl package for J2SE 5.0</rdfs:comment>
		<rdfs:comment xml:lang="OWLManchester">platform:implementsInterface some JavaxNetSslAPI</rdfs:comment>
	</owl:Class>
	<owl:Class rdf:about="&j2se-5_0;JavaxSecurityCertClassLibrary">
		<owl:equivalentClass rdf:resource="&j2se-1_4;JavaxSecurityCertClassLibrary"/>
		<rdfs:subClassOf rdf:resource="&java;JavaClassLibrary"/>
		<rdfs:comment xml:lang="en">JavaLibrary implementing the javax.security.cert package for J2SE 5.0</rdfs:comment>
		<rdfs:comment xml:lang="OWLManchester">platform:implementsInterface some JavaxSecurityCertAPI</rdfs:comment>
	</owl:Class>
	<owl:Class rdf:about="&j2se-5_0;JavaxSecurityAuthClassLibrary">
		<owl:equivalentClass rdf:resource="&j2se-1_4;JavaxSecurityAuthClassLibrary"/>
		<rdfs:subClassOf rdf:resource="&java;JavaClassLibrary"/>
		<rdfs:comment xml:lang="en">JavaLibrary implementing the javax.security.auth package for J2SE 5.0</rdfs:comment>
		<rdfs:comment xml:lang="OWLManchester">platform:implementsInterface some JavaxSecurityAuthAPI</rdfs:comment>
	</owl:Class>
	<owl:Class rdf:about="&j2se-5_0;JavaxSecurityAuthCallbackClassLibrary">
		<owl:equivalentClass rdf:resource="&j2se-1_4;JavaxSecurityAuthCallbackClassLibrary"/>
		<rdfs:subClassOf rdf:resource="&java;JavaClassLibrary"/>
		<rdfs:comment xml:lang="en">JavaLibrary implementing the javax.security.auth.callback package for J2SE 5.0</rdfs:comment>
		<rdfs:comment xml:lang="OWLManchester">platform:implementsInterface some JavaxSecurityAuthCallbackAPI</rdfs:comment>
	</owl:Class>
	<owl:Class rdf:about="&j2se-5_0;JavaxSecurityAuthX500ClassLibrary">
		<owl:equivalentClass rdf:resource="&j2se-1_4;JavaxSecurityAuthX500ClassLibrary"/>
		<rdfs:subClassOf rdf:resource="&java;JavaClassLibrary"/>
		<rdfs:comment xml:lang="en">JavaLibrary implementing the javax.security.auth.x500 package for J2SE 5.0</rdfs:comment>
		<rdfs:comment xml:lang="OWLManchester">platform:implementsInterface some JavaxSecurityAuthX500API</rdfs:comment>
	</owl:Class>
	<owl:Class rdf:about="&j2se-5_0;JavaxSecurityAuthKerberosClassLibrary">
		<owl:equivalentClass rdf:resource="&j2se-1_4;JavaxSecurityAuthKerberosClassLibrary"/>
		<rdfs:subClassOf rdf:resource="&java;JavaClassLibrary"/>
		<rdfs:comment xml:lang="en">JavaLibrary implementing the javax.security.auth.kerberos package for J2SE 5.0</rdfs:comment>
		<rdfs:comment xml:lang="OWLManchester">platform:implementsInterface some JavaxSecurityAuthKerberosAPI</rdfs:comment>
	</owl:Class>
	<owl:Class rdf:about="&j2se-5_0;JavaxSecurityAuthLoginClassLibrary">
		<rdfs:subClassOf rdf:resource="&j2se-1_4;JavaxSecurityAuthLoginClassLibrary"/>
		<rdfs:comment xml:lang="en">JavaLibrary implementing the javax.security.auth.login package for J2SE 5.0</rdfs:comment>
		<rdfs:comment xml:lang="OWLManchester">platform:implementsInterface some JavaxSecurityAuthLoginAPI</rdfs:comment>
	</owl:Class>
	<owl:Class rdf:about="&j2se-5_0;JavaxSecurityAuthSpiClassLibrary">
		<owl:equivalentClass rdf:resource="&j2se-1_4;JavaxSecurityAuthSpiClassLibrary"/>
		<rdfs:subClassOf rdf:resource="&java;JavaClassLibrary"/>
		<rdfs:comment xml:lang="en">JavaLibrary implementing the javax.security.auth.spi package for J2SE 5.0</rdfs:comment>
		<rdfs:comment xml:lang="OWLManchester">platform:implementsInterface some JavaxSecurityAuthSpiAPI</rdfs:comment>
	</owl:Class>
	<owl:Class rdf:about="&j2se-5_0;JavaxSecuritySaslClassLibrary">
		<rdfs:subClassOf rdf:resource="&java;JavaClassLibrary"/>
		<rdfs:comment xml:lang="en">JavaLibrary implementing the javax.security.sasl package for J2SE 5.0</rdfs:comment>
		<rdfs:comment xml:lang="OWLManchester">platform:implementsInterface some JavaxSecuritySaslAPI</rdfs:comment>
	</owl:Class>
	<owl:Class rdf:about="&j2se-5_0;JavaxAccessibilityClassLibrary">
		<rdfs:subClassOf rdf:resource="&j2se-1_4;JavaxAccessibilityClassLibrary"/>
		<rdfs:comment xml:lang="en">JavaLibrary implementing the javax.accessibility package for J2SE 5.0</rdfs:comment>
		<rdfs:comment xml:lang="OWLManchester">platform:implementsInterface some JavaxAccessibilityAPI</rdfs:comment>
	</owl:Class>
	<owl:Class rdf:about="&j2se-5_0;JavaxSwingClassLibrary">
		<rdfs:subClassOf rdf:resource="&j2se-1_4;JavaxSwingClassLibrary"/>
		<rdfs:comment xml:lang="en">JavaLibrary implementing the javax.swing package for J2SE 5.0</rdfs:comment>
		<rdfs:comment xml:lang="OWLManchester">platform:implementsInterface some JavaxSwingAPI</rdfs:comment>
	</owl:Class>
	<owl:Class rdf:about="&j2se-5_0;JavaxSwingTextClassLibrary">
		<rdfs:subClassOf rdf:resource="&j2se-1_4;JavaxSwingTextClassLibrary"/>
		<rdfs:comment xml:lang="en">JavaLibrary implementing the javax.swing.text package for J2SE 5.0</rdfs:comment>
		<rdfs:comment xml:lang="OWLManchester">platform:implementsInterface some JavaxSwingTextAPI</rdfs:comment>
	</owl:Class>
	<owl:Class rdf:about="&j2se-5_0;JavaxSwingTextHtmlClassLibrary">
		<rdfs:subClassOf rdf:resource="&j2se-1_4;JavaxSwingTextHtmlClassLibrary"/>
		<rdfs:comment xml:lang="en">JavaLibrary implementing the javax.swing.text.html package for J2SE 5.0</rdfs:comment>
		<rdfs:comment xml:lang="OWLManchester">platform:implementsInterface some JavaxSwingTextHtmlAPI</rdfs:comment>
	</owl:Class>
	<owl:Class rdf:about="&j2se-5_0;JavaxSwingTextHtmlParserClassLibrary">
		<owl:equivalentClass rdf:resource="&j2se-1_4;JavaxSwingTextHtmlParserClassLibrary"/>
		<rdfs:subClassOf rdf:resource="&java;JavaClassLibrary"/>
		<rdfs:comment xml:lang="en">JavaLibrary implementing the javax.swing.text.html.parser package for J2SE 5.0</rdfs:comment>
		<rdfs:comment xml:lang="OWLManchester">platform:implementsInterface some JavaxSwingTextHtmlParserAPI</rdfs:comment>
	</owl:Class>
	<owl:Class rdf:about="&j2se-5_0;JavaxSwingTextRtfClassLibrary">
		<owl:equivalentClass rdf:resource="&j2se-1_4;JavaxSwingTextRtfClassLibrary"/>
		<rdfs:subClassOf rdf:resource="&java;JavaClassLibrary"/>
		<rdfs:comment xml:lang="en">JavaLibrary implementing the javax.swing.text.rtf package for J2SE 5.0</rdfs:comment>
		<rdfs:comment xml:lang="OWLManchester">platform:implementsInterface some JavaxSwingTextRtfAPI</rdfs:comment>
	</owl:Class>
	<owl:Class rdf:about="&j2se-5_0;JavaxSwingEventClassLibrary">
		<rdfs:subClassOf rdf:resource="&j2se-1_4;JavaxSwingEventClassLibrary"/>
		<rdfs:comment xml:lang="en">JavaLibrary implementing the javax.swing.event package for J2SE 5.0</rdfs:comment>
		<rdfs:comment xml:lang="OWLManchester">platform:implementsInterface some JavaxSwingEventAPI</rdfs:comment>
	</owl:Class>
	<owl:Class rdf:about="&j2se-5_0;JavaxSwingColorchooserClassLibrary">
		<rdfs:subClassOf rdf:resource="&j2se-1_4;JavaxSwingColorchooserClassLibrary"/>
		<rdfs:comment xml:lang="en">JavaLibrary implementing the javax.swing.colorchooser package for J2SE 5.0</rdfs:comment>
		<rdfs:comment xml:lang="OWLManchester">platform:implementsInterface some JavaxSwingColorchooserAPI</rdfs:comment>
	</owl:Class>
	<owl:Class rdf:about="&j2se-5_0;JavaxSwingPlafClassLibrary">
		<rdfs:subClassOf rdf:resource="&j2se-1_4;JavaxSwingPlafClassLibrary"/>
		<rdfs:comment xml:lang="en">JavaLibrary implementing the javax.swing.plaf package for J2SE 5.0</rdfs:comment>
		<rdfs:comment xml:lang="OWLManchester">platform:implementsInterface some JavaxSwingPlafAPI</rdfs:comment>
	</owl:Class>
	<owl:Class rdf:about="&j2se-5_0;JavaxSwingPlafBasicClassLibrary">
		<rdfs:subClassOf rdf:resource="&j2se-1_4;JavaxSwingPlafBasicClassLibrary"/>
		<rdfs:comment xml:lang="en">JavaLibrary implementing the javax.swing.plaf.basic package for J2SE 5.0</rdfs:comment>
		<rdfs:comment xml:lang="OWLManchester">platform:implementsInterface some JavaxSwingPlafBasicAPI</rdfs:comment>
	</owl:Class>
	<owl:Class rdf:about="&j2se-5_0;JavaxSwingPlafMetalClassLibrary">
		<rdfs:subClassOf rdf:resource="&j2se-1_4;JavaxSwingPlafMetalClassLibrary"/>
		<rdfs:comment xml:lang="en">JavaLibrary implementing the javax.swing.plaf.metal package for J2SE 5.0</rdfs:comment>
		<rdfs:comment xml:lang="OWLManchester">platform:implementsInterface some JavaxSwingPlafMetalAPI</rdfs:comment>
	</owl:Class>
	<owl:Class rdf:about="&j2se-5_0;JavaxSwingPlafMultiClassLibrary">
		<rdfs:subClassOf rdf:resource="&j2se-1_4;JavaxSwingPlafMultiClassLibrary"/>
		<rdfs:comment xml:lang="en">JavaLibrary implementing the javax.swing.plaf.multi package for J2SE 5.0</rdfs:comment>
		<rdfs:comment xml:lang="OWLManchester">platform:implementsInterface some JavaxSwingPlafMultiAPI</rdfs:comment>
	</owl:Class>
	<owl:Class rdf:about="&j2se-5_0;JavaxSwingPlafSynthClassLibrary">
		<rdfs:subClassOf rdf:resource="&java;JavaClassLibrary"/>
		<rdfs:comment xml:lang="en">JavaLibrary implementing the javax.swing.plaf.synth package for J2SE 5.0</rdfs:comment>
		<rdfs:comment xml:lang="OWLManchester">platform:implementsInterface some JavaxSwingPlafSynthAPI</rdfs:comment>
	</owl:Class>
	<owl:Class rdf:about="&j2se-5_0;JavaxSwingTreeClassLibrary">
		<rdfs:subClassOf rdf:resource="&j2se-1_4;JavaxSwingTreeClassLibrary"/>
		<rdfs:comment xml:lang="en">JavaLibrary implementing the javax.swing.tree package for J2SE 5.0</rdfs:comment>
		<rdfs:comment xml:lang="OWLManchester">platform:implementsInterface some JavaxSwingTreeAPI</rdfs:comment>
	</owl:Class>
	<owl:Class rdf:about="&j2se-5_0;JavaxSwingBorderClassLibrary">
		<owl:equivalentClass rdf:resource="&j2se-1_4;JavaxSwingBorderClassLibrary"/>
		<rdfs:subClassOf rdf:resource="&java;JavaClassLibrary"/>
		<rdfs:comment xml:lang="en">JavaLibrary implementing the javax.swing.border package for J2SE 5.0</rdfs:comment>
		<rdfs:comment xml:lang="OWLManchester">platform:implementsInterface some JavaxSwingBorderAPI</rdfs:comment>
	</owl:Class>
	<owl:Class rdf:about="&j2se-5_0;JavaxSwingFilechooserClassLibrary">
		<owl:equivalentClass rdf:resource="&j2se-1_4;JavaxSwingFilechooserClassLibrary"/>
		<rdfs:subClassOf rdf:resource="&java;JavaClassLibrary"/>
		<rdfs:comment xml:lang="en">JavaLibrary implementing the javax.swing.filechooser package for J2SE 5.0</rdfs:comment>
		<rdfs:comment xml:lang="OWLManchester">platform:implementsInterface some JavaxSwingFilechooserAPI</rdfs:comment>
	</owl:Class>
	<owl:Class rdf:about="&j2se-5_0;JavaxSwingTableClassLibrary">
		<rdfs:subClassOf rdf:resource="&j2se-1_4;JavaxSwingTableClassLibrary"/>
		<rdfs:comment xml:lang="en">JavaLibrary implementing the javax.swing.table package for J2SE 5.0</rdfs:comment>
		<rdfs:comment xml:lang="OWLManchester">platform:implementsInterface some JavaxSwingTableAPI</rdfs:comment>
	</owl:Class>
	<owl:Class rdf:about="&j2se-5_0;JavaxSwingUndoClassLibrary">
		<owl:equivalentClass rdf:resource="&j2se-1_4;JavaxSwingUndoClassLibrary"/>
		<rdfs:subClassOf rdf:resource="&java;JavaClassLibrary"/>
		<rdfs:comment xml:lang="en">JavaLibrary implementing the javax.swing.undo package for J2SE 5.0</rdfs:comment>
		<rdfs:comment xml:lang="OWLManchester">platform:implementsInterface some JavaxSwingUndoAPI</rdfs:comment>
	</owl:Class>
	<owl:Class rdf:about="&j2se-5_0;JavaxManagementClassLibrary">
		<rdfs:subClassOf rdf:resource="&java;JavaClassLibrary"/>
		<rdfs:comment xml:lang="en">JavaLibrary implementing the javax.management package for J2SE 5.0</rdfs:comment>
		<rdfs:comment xml:lang="OWLManchester">platform:implementsInterface some JavaxManagementAPI</rdfs:comment>
	</owl:Class>
	<owl:Class rdf:about="&j2se-5_0;JavaxManagementOpenmbeanClassLibrary">
		<rdfs:subClassOf rdf:resource="&java;JavaClassLibrary"/>
		<rdfs:comment xml:lang="en">JavaLibrary implementing the javax.management.openmbean package for J2SE 5.0</rdfs:comment>
		<rdfs:comment xml:lang="OWLManchester">platform:implementsInterface some JavaxManagementOpenmbeanAPI</rdfs:comment>
	</owl:Class>
	<owl:Class rdf:about="&j2se-5_0;JavaxManagementLoadingClassLibrary">
		<rdfs:subClassOf rdf:resource="&java;JavaClassLibrary"/>
		<rdfs:comment xml:lang="en">JavaLibrary implementing the javax.management.loading package for J2SE 5.0</rdfs:comment>
		<rdfs:comment xml:lang="OWLManchester">platform:implementsInterface some JavaxManagementLoadingAPI</rdfs:comment>
	</owl:Class>
	<owl:Class rdf:about="&j2se-5_0;JavaxManagementModelmbeanClassLibrary">
		<rdfs:subClassOf rdf:resource="&java;JavaClassLibrary"/>
		<rdfs:comment xml:lang="en">JavaLibrary implementing the javax.management.modelmbean package for J2SE 5.0</rdfs:comment>
		<rdfs:comment xml:lang="OWLManchester">platform:implementsInterface some JavaxManagementModelmbeanAPI</rdfs:comment>
	</owl:Class>
	<owl:Class rdf:about="&j2se-5_0;JavaxManagementMonitorClassLibrary">
		<rdfs:subClassOf rdf:resource="&java;JavaClassLibrary"/>
		<rdfs:comment xml:lang="en">JavaLibrary implementing the javax.management.monitor package for J2SE 5.0</rdfs:comment>
		<rdfs:comment xml:lang="OWLManchester">platform:implementsInterface some JavaxManagementMonitorAPI</rdfs:comment>
	</owl:Class>
	<owl:Class rdf:about="&j2se-5_0;JavaxManagementRelationClassLibrary">
		<rdfs:subClassOf rdf:resource="&java;JavaClassLibrary"/>
		<rdfs:comment xml:lang="en">JavaLibrary implementing the javax.management.relation package for J2SE 5.0</rdfs:comment>
		<rdfs:comment xml:lang="OWLManchester">platform:implementsInterface some JavaxManagementRelationAPI</rdfs:comment>
	</owl:Class>
	<owl:Class rdf:about="&j2se-5_0;JavaxManagementRemoteClassLibrary">
		<rdfs:subClassOf rdf:resource="&java;JavaClassLibrary"/>
		<rdfs:comment xml:lang="en">JavaLibrary implementing the javax.management.remote package for J2SE 5.0</rdfs:comment>
		<rdfs:comment xml:lang="OWLManchester">platform:implementsInterface some JavaxManagementRemoteAPI</rdfs:comment>
	</owl:Class>
	<owl:Class rdf:about="&j2se-5_0;JavaxManagementRemoteRmiClassLibrary">
		<rdfs:subClassOf rdf:resource="&java;JavaClassLibrary"/>
		<rdfs:comment xml:lang="en">JavaLibrary implementing the javax.management.remote.rmi package for J2SE 5.0</rdfs:comment>
		<rdfs:comment xml:lang="OWLManchester">platform:implementsInterface some JavaxManagementRemoteRmiAPI</rdfs:comment>
	</owl:Class>
	<owl:Class rdf:about="&j2se-5_0;JavaxManagementTimerClassLibrary">
		<rdfs:subClassOf rdf:resource="&java;JavaClassLibrary"/>
		<rdfs:comment xml:lang="en">JavaLibrary implementing the javax.management.timer package for J2SE 5.0</rdfs:comment>
		<rdfs:comment xml:lang="OWLManchester">platform:implementsInterface some JavaxManagementTimerAPI</rdfs:comment>
	</owl:Class>
	<owl:Class rdf:about="&j2se-5_0;JavaxActivityClassLibrary">
		<rdfs:subClassOf rdf:resource="&java;JavaClassLibrary"/>
		<rdfs:comment xml:lang="en">JavaLibrary implementing the javax.activity package for J2SE 5.0</rdfs:comment>
		<rdfs:comment xml:lang="OWLManchester">platform:implementsInterface some JavaxActivityAPI</rdfs:comment>
	</owl:Class>
	<owl:Class rdf:about="&j2se-5_0;JavaxImageioClassLibrary">
		<owl:equivalentClass rdf:resource="&j2se-1_4;JavaxImageioClassLibrary"/>
		<rdfs:subClassOf rdf:resource="&java;JavaClassLibrary"/>
		<rdfs:comment xml:lang="en">JavaLibrary implementing the javax.imageio package for J2SE 5.0</rdfs:comment>
		<rdfs:comment xml:lang="OWLManchester">platform:implementsInterface some JavaxImageioAPI</rdfs:comment>
	</owl:Class>
	<owl:Class rdf:about="&j2se-5_0;JavaxImageioMetadataClassLibrary">
		<rdfs:subClassOf rdf:resource="&j2se-1_4;JavaxImageioMetadataClassLibrary"/>
		<rdfs:comment xml:lang="en">JavaLibrary implementing the javax.imageio.metadata package for J2SE 5.0</rdfs:comment>
		<rdfs:comment xml:lang="OWLManchester">platform:implementsInterface some JavaxImageioMetadataAPI</rdfs:comment>
	</owl:Class>
	<owl:Class rdf:about="&j2se-5_0;JavaxImageioEventClassLibrary">
		<owl:equivalentClass rdf:resource="&j2se-1_4;JavaxImageioEventClassLibrary"/>
		<rdfs:subClassOf rdf:resource="&java;JavaClassLibrary"/>
		<rdfs:comment xml:lang="en">JavaLibrary implementing the javax.imageio.event package for J2SE 5.0</rdfs:comment>
		<rdfs:comment xml:lang="OWLManchester">platform:implementsInterface some JavaxImageioEventAPI</rdfs:comment>
	</owl:Class>
	<owl:Class rdf:about="&j2se-5_0;JavaxImageioPluginsBmpClassLibrary">
		<rdfs:subClassOf rdf:resource="&java;JavaClassLibrary"/>
		<rdfs:comment xml:lang="en">JavaLibrary implementing the javax.imageio.plugins.bmp package for J2SE 5.0</rdfs:comment>
		<rdfs:comment xml:lang="OWLManchester">platform:implementsInterface some JavaxImageioPluginsBmpAPI</rdfs:comment>
	</owl:Class>
	<owl:Class rdf:about="&j2se-5_0;JavaxImageioPluginsJpegClassLibrary">
		<owl:equivalentClass rdf:resource="&j2se-1_4;JavaxImageioPluginsJpegClassLibrary"/>
		<rdfs:subClassOf rdf:resource="&java;JavaClassLibrary"/>
		<rdfs:comment xml:lang="en">JavaLibrary implementing the javax.imageio.plugins.jpeg package for J2SE 5.0</rdfs:comment>
		<rdfs:comment xml:lang="OWLManchester">platform:implementsInterface some JavaxImageioPluginsJpegAPI</rdfs:comment>
	</owl:Class>
	<owl:Class rdf:about="&j2se-5_0;JavaxImageioStreamClassLibrary">
		<owl:equivalentClass rdf:resource="&j2se-1_4;JavaxImageioStreamClassLibrary"/>
		<rdfs:subClassOf rdf:resource="&java;JavaClassLibrary"/>
		<rdfs:comment xml:lang="en">JavaLibrary implementing the javax.imageio.stream package for J2SE 5.0</rdfs:comment>
		<rdfs:comment xml:lang="OWLManchester">platform:implementsInterface some JavaxImageioStreamAPI</rdfs:comment>
	</owl:Class>
	<owl:Class rdf:about="&j2se-5_0;JavaxImageioSpiClassLibrary">
		<owl:equivalentClass rdf:resource="&j2se-1_4;JavaxImageioSpiClassLibrary"/>
		<rdfs:subClassOf rdf:resource="&java;JavaClassLibrary"/>
		<rdfs:comment xml:lang="en">JavaLibrary implementing the javax.imageio.spi package for J2SE 5.0</rdfs:comment>
		<rdfs:comment xml:lang="OWLManchester">platform:implementsInterface some JavaxImageioSpiAPI</rdfs:comment>
	</owl:Class>
	<owl:Class rdf:about="&j2se-5_0;JavaxNamingClassLibrary">
		<rdfs:subClassOf rdf:resource="&j2se-1_4;JavaxNamingClassLibrary"/>
		<rdfs:comment xml:lang="en">JavaLibrary implementing the javax.naming package for J2SE 5.0</rdfs:comment>
		<rdfs:comment xml:lang="OWLManchester">platform:implementsInterface some JavaxNamingAPI</rdfs:comment>
	</owl:Class>
	<owl:Class rdf:about="&j2se-5_0;JavaxNamingDirectoryClassLibrary">
		<rdfs:subClassOf rdf:resource="&j2se-1_4;JavaxNamingDirectoryClassLibrary"/>
		<rdfs:comment xml:lang="en">JavaLibrary implementing the javax.naming.directory package for J2SE 5.0</rdfs:comment>
		<rdfs:comment xml:lang="OWLManchester">platform:implementsInterface some JavaxNamingDirectoryAPI</rdfs:comment>
	</owl:Class>
	<owl:Class rdf:about="&j2se-5_0;JavaxNamingEventClassLibrary">
		<owl:equivalentClass rdf:resource="&j2se-1_4;JavaxNamingEventClassLibrary"/>
		<rdfs:subClassOf rdf:resource="&java;JavaClassLibrary"/>
		<rdfs:comment xml:lang="en">JavaLibrary implementing the javax.naming.event package for J2SE 5.0</rdfs:comment>
		<rdfs:comment xml:lang="OWLManchester">platform:implementsInterface some JavaxNamingEventAPI</rdfs:comment>
	</owl:Class>
	<owl:Class rdf:about="&j2se-5_0;JavaxNamingLdapClassLibrary">
		<rdfs:subClassOf rdf:resource="&j2se-1_4;JavaxNamingLdapClassLibrary"/>
		<rdfs:comment xml:lang="en">JavaLibrary implementing the javax.naming.ldap package for J2SE 5.0</rdfs:comment>
		<rdfs:comment xml:lang="OWLManchester">platform:implementsInterface some JavaxNamingLdapAPI</rdfs:comment>
	</owl:Class>
	<owl:Class rdf:about="&j2se-5_0;JavaxNamingSpiClassLibrary">
		<owl:equivalentClass rdf:resource="&j2se-1_4;JavaxNamingSpiClassLibrary"/>
		<rdfs:subClassOf rdf:resource="&java;JavaClassLibrary"/>
		<rdfs:comment xml:lang="en">JavaLibrary implementing the javax.naming.spi package for J2SE 5.0</rdfs:comment>
		<rdfs:comment xml:lang="OWLManchester">platform:implementsInterface some JavaxNamingSpiAPI</rdfs:comment>
	</owl:Class>
	<owl:Class rdf:about="&j2se-5_0;JavaxPrintClassLibrary">
		<owl:equivalentClass rdf:resource="&j2se-1_4;JavaxPrintClassLibrary"/>
		<rdfs:subClassOf rdf:resource="&java;JavaClassLibrary"/>
		<rdfs:comment xml:lang="en">JavaLibrary implementing the javax.print package for J2SE 5.0</rdfs:comment>
		<rdfs:comment xml:lang="OWLManchester">platform:implementsInterface some JavaxPrintAPI</rdfs:comment>
	</owl:Class>
	<owl:Class rdf:about="&j2se-5_0;JavaxPrintAttributeClassLibrary">
		<owl:equivalentClass rdf:resource="&j2se-1_4;JavaxPrintAttributeClassLibrary"/>
		<rdfs:subClassOf rdf:resource="&java;JavaClassLibrary"/>
		<rdfs:comment xml:lang="en">JavaLibrary implementing the javax.print.attribute package for J2SE 5.0</rdfs:comment>
		<rdfs:comment xml:lang="OWLManchester">platform:implementsInterface some JavaxPrintAttributeAPI</rdfs:comment>
	</owl:Class>
	<owl:Class rdf:about="&j2se-5_0;JavaxPrintAttributeStandardClassLibrary">
		<rdfs:subClassOf rdf:resource="&j2se-1_4;JavaxPrintAttributeStandardClassLibrary"/>
		<rdfs:comment xml:lang="en">JavaLibrary implementing the javax.print.attribute.standard package for J2SE 5.0</rdfs:comment>
		<rdfs:comment xml:lang="OWLManchester">platform:implementsInterface some JavaxPrintAttributeStandardAPI</rdfs:comment>
	</owl:Class>
	<owl:Class rdf:about="&j2se-5_0;JavaxPrintEventClassLibrary">
		<owl:equivalentClass rdf:resource="&j2se-1_4;JavaxPrintEventClassLibrary"/>
		<rdfs:subClassOf rdf:resource="&java;JavaClassLibrary"/>
		<rdfs:comment xml:lang="en">JavaLibrary implementing the javax.print.event package for J2SE 5.0</rdfs:comment>
		<rdfs:comment xml:lang="OWLManchester">platform:implementsInterface some JavaxPrintEventAPI</rdfs:comment>
	</owl:Class>
	<owl:Class rdf:about="&j2se-5_0;JavaxRmiClassLibrary">
		<owl:equivalentClass rdf:resource="&j2se-1_4;JavaxRmiClassLibrary"/>
		<rdfs:subClassOf rdf:resource="&java;JavaClassLibrary"/>
		<rdfs:comment xml:lang="en">JavaLibrary implementing the javax.rmi package for J2SE 5.0</rdfs:comment>
		<rdfs:comment xml:lang="OWLManchester">platform:implementsInterface some JavaxRmiAPI</rdfs:comment>
	</owl:Class>
	<owl:Class rdf:about="&j2se-5_0;JavaxRmiCORBAClassLibrary">
		<rdfs:subClassOf rdf:resource="&j2se-1_4;JavaxRmiCORBAClassLibrary"/>
		<rdfs:comment xml:lang="en">JavaLibrary implementing the javax.rmi.CORBA package for J2SE 5.0</rdfs:comment>
		<rdfs:comment xml:lang="OWLManchester">platform:implementsInterface some JavaxRmiCORBAAPI</rdfs:comment>
	</owl:Class>
	<owl:Class rdf:about="&j2se-5_0;JavaxRmiSslClassLibrary">
		<rdfs:subClassOf rdf:resource="&java;JavaClassLibrary"/>
		<rdfs:comment xml:lang="en">JavaLibrary implementing the javax.rmi.ssl package for J2SE 5.0</rdfs:comment>
		<rdfs:comment xml:lang="OWLManchester">platform:implementsInterface some JavaxRmiSslAPI</rdfs:comment>
	</owl:Class>
	<owl:Class rdf:about="&j2se-5_0;JavaxSoundMidiClassLibrary">
		<rdfs:subClassOf rdf:resource="&java;JavaClassLibrary"/>
		<rdfs:comment xml:lang="en">JavaLibrary implementing the javax.sound.midi package for J2SE 5.0</rdfs:comment>
		<rdfs:comment xml:lang="OWLManchester">platform:implementsInterface some JavaxSoundMidiAPI</rdfs:comment>
	</owl:Class>
	<owl:Class rdf:about="&j2se-5_0;JavaxSoundMidiSpiClassLibrary">
		<owl:equivalentClass rdf:resource="&j2se-1_4;JavaxSoundMidiSpiClassLibrary"/>
		<rdfs:subClassOf rdf:resource="&java;JavaClassLibrary"/>
		<rdfs:comment xml:lang="en">JavaLibrary implementing the javax.sound.midi.spi package for J2SE 5.0</rdfs:comment>
		<rdfs:comment xml:lang="OWLManchester">platform:implementsInterface some JavaxSoundMidiSpiAPI</rdfs:comment>
	</owl:Class>
	<owl:Class rdf:about="&j2se-5_0;JavaxSoundSampledClassLibrary">
		<rdfs:subClassOf rdf:resource="&j2se-1_4;JavaxSoundSampledClassLibrary"/>
		<rdfs:comment xml:lang="en">JavaLibrary implementing the javax.sound.sampled package for J2SE 5.0</rdfs:comment>
		<rdfs:comment xml:lang="OWLManchester">platform:implementsInterface some JavaxSoundSampledAPI</rdfs:comment>
	</owl:Class>
	<owl:Class rdf:about="&j2se-5_0;JavaxSoundSampledSpiClassLibrary">
		<owl:equivalentClass rdf:resource="&j2se-1_4;JavaxSoundSampledSpiClassLibrary"/>
		<rdfs:subClassOf rdf:resource="&java;JavaClassLibrary"/>
		<rdfs:comment xml:lang="en">JavaLibrary implementing the javax.sound.sampled.spi package for J2SE 5.0</rdfs:comment>
		<rdfs:comment xml:lang="OWLManchester">platform:implementsInterface some JavaxSoundSampledSpiAPI</rdfs:comment>
	</owl:Class>
	<owl:Class rdf:about="&j2se-5_0;JavaxSqlClassLibrary">
		<owl:equivalentClass rdf:resource="&j2se-1_4;JavaxSqlClassLibrary"/>
		<rdfs:subClassOf rdf:resource="&java;JavaClassLibrary"/>
		<rdfs:comment xml:lang="en">JavaLibrary implementing the javax.sql package for J2SE 5.0</rdfs:comment>
		<rdfs:comment xml:lang="OWLManchester">platform:implementsInterface some JavaxSqlAPI</rdfs:comment>
	</owl:Class>
	<owl:Class rdf:about="&j2se-5_0;JavaxSqlRowsetClassLibrary">
		<rdfs:subClassOf rdf:resource="&java;JavaClassLibrary"/>
		<rdfs:comment xml:lang="en">JavaLibrary implementing the javax.sql.rowset package for J2SE 5.0</rdfs:comment>
		<rdfs:comment xml:lang="OWLManchester">platform:implementsInterface some JavaxSqlRowsetAPI</rdfs:comment>
	</owl:Class>
	<owl:Class rdf:about="&j2se-5_0;JavaxSqlRowsetSpiClassLibrary">
		<rdfs:subClassOf rdf:resource="&java;JavaClassLibrary"/>
		<rdfs:comment xml:lang="en">JavaLibrary implementing the javax.sql.rowset.spi package for J2SE 5.0</rdfs:comment>
		<rdfs:comment xml:lang="OWLManchester">platform:implementsInterface some JavaxSqlRowsetSpiAPI</rdfs:comment>
	</owl:Class>
	<owl:Class rdf:about="&j2se-5_0;JavaxSqlRowsetSerialClassLibrary">
		<rdfs:subClassOf rdf:resource="&java;JavaClassLibrary"/>
		<rdfs:comment xml:lang="en">JavaLibrary implementing the javax.sql.rowset.serial package for J2SE 5.0</rdfs:comment>
		<rdfs:comment xml:lang="OWLManchester">platform:implementsInterface some JavaxSqlRowsetSerialAPI</rdfs:comment>
	</owl:Class>
	<owl:Class rdf:about="&j2se-5_0;JavaxTransactionClassLibrary">
		<owl:equivalentClass rdf:resource="&j2se-1_4;JavaxTransactionClassLibrary"/>
		<rdfs:subClassOf rdf:resource="&java;JavaClassLibrary"/>
		<rdfs:comment xml:lang="en">JavaLibrary implementing the javax.transaction package for J2SE 5.0</rdfs:comment>
		<rdfs:comment xml:lang="OWLManchester">platform:implementsInterface some JavaxTransactionAPI</rdfs:comment>
	</owl:Class>
	<owl:Class rdf:about="&j2se-5_0;JavaxTransactionXaClassLibrary">
		<owl:equivalentClass rdf:resource="&j2se-1_4;JavaxTransactionXaClassLibrary"/>
		<rdfs:subClassOf rdf:resource="&java;JavaClassLibrary"/>
		<rdfs:comment xml:lang="en">JavaLibrary implementing the javax.transaction.xa package for J2SE 5.0</rdfs:comment>
		<rdfs:comment xml:lang="OWLManchester">platform:implementsInterface some JavaxTransactionXaAPI</rdfs:comment>
	</owl:Class>
	<owl:Class rdf:about="&j2se-5_0;JavaxXmlClassLibrary">
		<rdfs:subClassOf rdf:resource="&java;JavaClassLibrary"/>
		<rdfs:comment xml:lang="en">JavaLibrary implementing the javax.xml package for J2SE 5.0</rdfs:comment>
		<rdfs:comment xml:lang="OWLManchester">platform:implementsInterface some JavaxXmlAPI</rdfs:comment>
	</owl:Class>
	<owl:Class rdf:about="&j2se-5_0;JavaxXmlDatatypeClassLibrary">
		<rdfs:subClassOf rdf:resource="&java;JavaClassLibrary"/>
		<rdfs:comment xml:lang="en">JavaLibrary implementing the javax.xml.datatype package for J2SE 5.0</rdfs:comment>
		<rdfs:comment xml:lang="OWLManchester">platform:implementsInterface some JavaxXmlDatatypeAPI</rdfs:comment>
	</owl:Class>
	<owl:Class rdf:about="&j2se-5_0;JavaxXmlNamespaceClassLibrary">
		<rdfs:subClassOf rdf:resource="&java;JavaClassLibrary"/>
		<rdfs:comment xml:lang="en">JavaLibrary implementing the javax.xml.namespace package for J2SE 5.0</rdfs:comment>
		<rdfs:comment xml:lang="OWLManchester">platform:implementsInterface some JavaxXmlNamespaceAPI</rdfs:comment>
	</owl:Class>
	<owl:Class rdf:about="&j2se-5_0;JavaxXmlTransformClassLibrary">
		<rdfs:subClassOf rdf:resource="&j2se-1_4;JavaxXmlTransformClassLibrary"/>
		<rdfs:comment xml:lang="en">JavaLibrary implementing the javax.xml.transform package for J2SE 5.0</rdfs:comment>
		<rdfs:comment xml:lang="OWLManchester">platform:implementsInterface some JavaxXmlTransformAPI</rdfs:comment>
	</owl:Class>
	<owl:Class rdf:about="&j2se-5_0;JavaxXmlTransformDomClassLibrary">
		<rdfs:subClassOf rdf:resource="&j2se-1_4;JavaxXmlTransformDomClassLibrary"/>
		<rdfs:comment xml:lang="en">JavaLibrary implementing the javax.xml.transform.dom package for J2SE 5.0</rdfs:comment>
		<rdfs:comment xml:lang="OWLManchester">platform:implementsInterface some JavaxXmlTransformDomAPI</rdfs:comment>
	</owl:Class>
	<owl:Class rdf:about="&j2se-5_0;JavaxXmlTransformSaxClassLibrary">
		<rdfs:subClassOf rdf:resource="&j2se-1_4;JavaxXmlTransformSaxClassLibrary"/>
		<rdfs:comment xml:lang="en">JavaLibrary implementing the javax.xml.transform.sax package for J2SE 5.0</rdfs:comment>
		<rdfs:comment xml:lang="OWLManchester">platform:implementsInterface some JavaxXmlTransformSaxAPI</rdfs:comment>
	</owl:Class>
	<owl:Class rdf:about="&j2se-5_0;JavaxXmlTransformStreamClassLibrary">
		<owl:equivalentClass rdf:resource="&j2se-1_4;JavaxXmlTransformStreamClassLibrary"/>
		<rdfs:subClassOf rdf:resource="&java;JavaClassLibrary"/>
		<rdfs:comment xml:lang="en">JavaLibrary implementing the javax.xml.transform.stream package for J2SE 5.0</rdfs:comment>
		<rdfs:comment xml:lang="OWLManchester">platform:implementsInterface some JavaxXmlTransformStreamAPI</rdfs:comment>
	</owl:Class>
	<owl:Class rdf:about="&j2se-5_0;JavaxXmlValidationClassLibrary">
		<rdfs:subClassOf rdf:resource="&java;JavaClassLibrary"/>
		<rdfs:comment xml:lang="en">JavaLibrary implementing the javax.xml.validation package for J2SE 5.0</rdfs:comment>
		<rdfs:comment xml:lang="OWLManchester">platform:implementsInterface some JavaxXmlValidationAPI</rdfs:comment>
	</owl:Class>
	<owl:Class rdf:about="&j2se-5_0;JavaxXmlXpathClassLibrary">
		<rdfs:subClassOf rdf:resource="&java;JavaClassLibrary"/>
		<rdfs:comment xml:lang="en">JavaLibrary implementing the javax.xml.xpath package for J2SE 5.0</rdfs:comment>
		<rdfs:comment xml:lang="OWLManchester">platform:implementsInterface some JavaxXmlXpathAPI</rdfs:comment>
	</owl:Class>
	<owl:Class rdf:about="&j2se-5_0;JavaxXmlParsersClassLibrary">
		<rdfs:subClassOf rdf:resource="&j2se-1_4;JavaxXmlParsersClassLibrary"/>
		<rdfs:comment xml:lang="en">JavaLibrary implementing the javax.xml.parsers package for J2SE 5.0</rdfs:comment>
		<rdfs:comment xml:lang="OWLManchester">platform:implementsInterface some JavaxXmlParsersAPI</rdfs:comment>
	</owl:Class>
	<owl:Class rdf:about="&j2se-5_0;JavaLangClassLibrary">
		<rdfs:subClassOf rdf:resource="&j2se-1_4;JavaLangClassLibrary"/>
		<rdfs:comment xml:lang="en">JavaLibrary implementing the java.lang package for J2SE 5.0</rdfs:comment>
		<rdfs:comment xml:lang="OWLManchester">platform:implementsInterface some JavaLangAPI</rdfs:comment>
	</owl:Class>
	<owl:Class rdf:about="&j2se-5_0;JavaLangReflectClassLibrary">
		<rdfs:subClassOf rdf:resource="&j2se-1_4;JavaLangReflectClassLibrary"/>
		<rdfs:comment xml:lang="en">JavaLibrary implementing the java.lang.reflect package for J2SE 5.0</rdfs:comment>
		<rdfs:comment xml:lang="OWLManchester">platform:implementsInterface some JavaLangReflectAPI</rdfs:comment>
	</owl:Class>
	<owl:Class rdf:about="&j2se-5_0;JavaLangAnnotationClassLibrary">
		<rdfs:subClassOf rdf:resource="&java;JavaClassLibrary"/>
		<rdfs:comment xml:lang="en">JavaLibrary implementing the java.lang.annotation package for J2SE 5.0</rdfs:comment>
		<rdfs:comment xml:lang="OWLManchester">platform:implementsInterface some JavaLangAnnotationAPI</rdfs:comment>
	</owl:Class>
	<owl:Class rdf:about="&j2se-5_0;JavaLangInstrumentClassLibrary">
		<rdfs:subClassOf rdf:resource="&java;JavaClassLibrary"/>
		<rdfs:comment xml:lang="en">JavaLibrary implementing the java.lang.instrument package for J2SE 5.0</rdfs:comment>
		<rdfs:comment xml:lang="OWLManchester">platform:implementsInterface some JavaLangInstrumentAPI</rdfs:comment>
	</owl:Class>
	<owl:Class rdf:about="&j2se-5_0;JavaLangManagementClassLibrary">
		<rdfs:subClassOf rdf:resource="&java;JavaClassLibrary"/>
		<rdfs:comment xml:lang="en">JavaLibrary implementing the java.lang.management package for J2SE 5.0</rdfs:comment>
		<rdfs:comment xml:lang="OWLManchester">platform:implementsInterface some JavaLangManagementAPI</rdfs:comment>
	</owl:Class>
	<owl:Class rdf:about="&j2se-5_0;JavaLangRefClassLibrary">
		<owl:equivalentClass rdf:resource="&j2se-1_4;JavaLangRefClassLibrary"/>
		<rdfs:subClassOf rdf:resource="&java;JavaClassLibrary"/>
		<rdfs:comment xml:lang="en">JavaLibrary implementing the java.lang.ref package for J2SE 5.0</rdfs:comment>
		<rdfs:comment xml:lang="OWLManchester">platform:implementsInterface some JavaLangRefAPI</rdfs:comment>
	</owl:Class>
	<owl:Class rdf:about="&j2se-5_0;JavaSecurityClassLibrary">
		<rdfs:subClassOf rdf:resource="&j2se-1_4;JavaSecurityClassLibrary"/>
		<rdfs:comment xml:lang="en">JavaLibrary implementing the java.security package for J2SE 5.0</rdfs:comment>
		<rdfs:comment xml:lang="OWLManchester">platform:implementsInterface some JavaSecurityAPI</rdfs:comment>
	</owl:Class>
	<owl:Class rdf:about="&j2se-5_0;JavaSecuritySpecClassLibrary">
		<rdfs:subClassOf rdf:resource="&j2se-1_4;JavaSecuritySpecClassLibrary"/>
		<rdfs:comment xml:lang="en">JavaLibrary implementing the java.security.spec package for J2SE 5.0</rdfs:comment>
		<rdfs:comment xml:lang="OWLManchester">platform:implementsInterface some JavaSecuritySpecAPI</rdfs:comment>
	</owl:Class>
	<owl:Class rdf:about="&j2se-5_0;JavaSecurityCertClassLibrary">
		<rdfs:subClassOf rdf:resource="&java;JavaClassLibrary"/>
		<rdfs:comment xml:lang="en">JavaLibrary implementing the java.security.cert package for J2SE 5.0</rdfs:comment>
		<rdfs:comment xml:lang="OWLManchester">platform:implementsInterface some JavaSecurityCertAPI</rdfs:comment>
	</owl:Class>
	<owl:Class rdf:about="&j2se-5_0;JavaSecurityAclClassLibrary">
		<owl:equivalentClass rdf:resource="&j2se-1_4;JavaSecurityAclClassLibrary"/>
		<rdfs:subClassOf rdf:resource="&java;JavaClassLibrary"/>
		<rdfs:comment xml:lang="en">JavaLibrary implementing the java.security.acl package for J2SE 5.0</rdfs:comment>
		<rdfs:comment xml:lang="OWLManchester">platform:implementsInterface some JavaSecurityAclAPI</rdfs:comment>
	</owl:Class>
	<owl:Class rdf:about="&j2se-5_0;JavaSecurityInterfacesClassLibrary">
		<rdfs:subClassOf rdf:resource="&j2se-1_4;JavaSecurityInterfacesClassLibrary"/>
		<rdfs:comment xml:lang="en">JavaLibrary implementing the java.security.interfaces package for J2SE 5.0</rdfs:comment>
		<rdfs:comment xml:lang="OWLManchester">platform:implementsInterface some JavaSecurityInterfacesAPI</rdfs:comment>
	</owl:Class>
	<owl:Class rdf:about="&j2se-5_0;JavaMathClassLibrary">
		<rdfs:subClassOf rdf:resource="&j2se-1_4;JavaMathClassLibrary"/>
		<rdfs:comment xml:lang="en">JavaLibrary implementing the java.math package for J2SE 5.0</rdfs:comment>
		<rdfs:comment xml:lang="OWLManchester">platform:implementsInterface some JavaMathAPI</rdfs:comment>
	</owl:Class>
	<owl:Class rdf:about="&j2se-5_0;JavaNioClassLibrary">
		<rdfs:subClassOf rdf:resource="&j2se-1_4;JavaNioClassLibrary"/>
		<rdfs:comment xml:lang="en">JavaLibrary implementing the java.nio package for J2SE 5.0</rdfs:comment>
		<rdfs:comment xml:lang="OWLManchester">platform:implementsInterface some JavaNioAPI</rdfs:comment>
	</owl:Class>
	<owl:Class rdf:about="&j2se-5_0;JavaNioChannelsClassLibrary">
		<rdfs:subClassOf rdf:resource="&j2se-1_4;JavaNioChannelsClassLibrary"/>
		<rdfs:comment xml:lang="en">JavaLibrary implementing the java.nio.channels package for J2SE 5.0</rdfs:comment>
		<rdfs:comment xml:lang="OWLManchester">platform:implementsInterface some JavaNioChannelsAPI</rdfs:comment>
	</owl:Class>
	<owl:Class rdf:about="&j2se-5_0;JavaNioChannelsSpiClassLibrary">
		<rdfs:subClassOf rdf:resource="&j2se-1_4;JavaNioChannelsSpiClassLibrary"/>
		<rdfs:comment xml:lang="en">JavaLibrary implementing the java.nio.channels.spi package for J2SE 5.0</rdfs:comment>
		<rdfs:comment xml:lang="OWLManchester">platform:implementsInterface some JavaNioChannelsSpiAPI</rdfs:comment>
	</owl:Class>
	<owl:Class rdf:about="&j2se-5_0;JavaNioCharsetClassLibrary">
		<rdfs:subClassOf rdf:resource="&j2se-1_4;JavaNioCharsetClassLibrary"/>
		<rdfs:comment xml:lang="en">JavaLibrary implementing the java.nio.charset package for J2SE 5.0</rdfs:comment>
		<rdfs:comment xml:lang="OWLManchester">platform:implementsInterface some JavaNioCharsetAPI</rdfs:comment>
	</owl:Class>
	<owl:Class rdf:about="&j2se-5_0;JavaNioCharsetSpiClassLibrary">
		<owl:equivalentClass rdf:resource="&j2se-1_4;JavaNioCharsetSpiClassLibrary"/>
		<rdfs:subClassOf rdf:resource="&java;JavaClassLibrary"/>
		<rdfs:comment xml:lang="en">JavaLibrary implementing the java.nio.charset.spi package for J2SE 5.0</rdfs:comment>
		<rdfs:comment xml:lang="OWLManchester">platform:implementsInterface some JavaNioCharsetSpiAPI</rdfs:comment>
	</owl:Class>
	<owl:Class rdf:about="&j2se-5_0;JavaIoClassLibrary">
		<rdfs:subClassOf rdf:resource="&j2se-1_4;JavaIoClassLibrary"/>
		<rdfs:comment xml:lang="en">JavaLibrary implementing the java.io package for J2SE 5.0</rdfs:comment>
		<rdfs:comment xml:lang="OWLManchester">platform:implementsInterface some JavaIoAPI</rdfs:comment>
	</owl:Class>
	<owl:Class rdf:about="&j2se-5_0;JavaNetClassLibrary">
		<rdfs:subClassOf rdf:resource="&j2se-1_4;JavaNetClassLibrary"/>
		<rdfs:comment xml:lang="en">JavaLibrary implementing the java.net package for J2SE 5.0</rdfs:comment>
		<rdfs:comment xml:lang="OWLManchester">platform:implementsInterface some JavaNetAPI</rdfs:comment>
	</owl:Class>
	<owl:Class rdf:about="&j2se-5_0;JavaUtilClassLibrary">
		<rdfs:subClassOf rdf:resource="&j2se-1_4;JavaUtilClassLibrary"/>
		<rdfs:comment xml:lang="en">JavaLibrary implementing the java.util package for J2SE 5.0</rdfs:comment>
		<rdfs:comment xml:lang="OWLManchester">platform:implementsInterface some JavaUtilAPI</rdfs:comment>
	</owl:Class>
	<owl:Class rdf:about="&j2se-5_0;JavaUtilRegexClassLibrary">
		<rdfs:subClassOf rdf:resource="&j2se-1_4;JavaUtilRegexClassLibrary"/>
		<rdfs:comment xml:lang="en">JavaLibrary implementing the java.util.regex package for J2SE 5.0</rdfs:comment>
		<rdfs:comment xml:lang="OWLManchester">platform:implementsInterface some JavaUtilRegexAPI</rdfs:comment>
	</owl:Class>
	<owl:Class rdf:about="&j2se-5_0;JavaUtilConcurrentClassLibrary">
		<rdfs:subClassOf rdf:resource="&java;JavaClassLibrary"/>
		<rdfs:comment xml:lang="en">JavaLibrary implementing the java.util.concurrent package for J2SE 5.0</rdfs:comment>
		<rdfs:comment xml:lang="OWLManchester">platform:implementsInterface some JavaUtilConcurrentAPI</rdfs:comment>
	</owl:Class>
	<owl:Class rdf:about="&j2se-5_0;JavaUtilConcurrentAtomicClassLibrary">
		<rdfs:subClassOf rdf:resource="&java;JavaClassLibrary"/>
		<rdfs:comment xml:lang="en">JavaLibrary implementing the java.util.concurrent.atomic package for J2SE 5.0</rdfs:comment>
		<rdfs:comment xml:lang="OWLManchester">platform:implementsInterface some JavaUtilConcurrentAtomicAPI</rdfs:comment>
	</owl:Class>
	<owl:Class rdf:about="&j2se-5_0;JavaUtilConcurrentLocksClassLibrary">
		<rdfs:subClassOf rdf:resource="&java;JavaClassLibrary"/>
		<rdfs:comment xml:lang="en">JavaLibrary implementing the java.util.concurrent.locks package for J2SE 5.0</rdfs:comment>
		<rdfs:comment xml:lang="OWLManchester">platform:implementsInterface some JavaUtilConcurrentLocksAPI</rdfs:comment>
	</owl:Class>
	<owl:Class rdf:about="&j2se-5_0;JavaUtilJarClassLibrary">
		<rdfs:subClassOf rdf:resource="&j2se-1_4;JavaUtilJarClassLibrary"/>
		<rdfs:comment xml:lang="en">JavaLibrary implementing the java.util.jar package for J2SE 5.0</rdfs:comment>
		<rdfs:comment xml:lang="OWLManchester">platform:implementsInterface some JavaUtilJarAPI</rdfs:comment>
	</owl:Class>
	<owl:Class rdf:about="&j2se-5_0;JavaUtilZipClassLibrary">
		<rdfs:subClassOf rdf:resource="&j2se-1_4;JavaUtilZipClassLibrary"/>
		<rdfs:comment xml:lang="en">JavaLibrary implementing the java.util.zip package for J2SE 5.0</rdfs:comment>
		<rdfs:comment xml:lang="OWLManchester">platform:implementsInterface some JavaUtilZipAPI</rdfs:comment>
	</owl:Class>
	<owl:Class rdf:about="&j2se-5_0;JavaUtilLoggingClassLibrary">
		<rdfs:subClassOf rdf:resource="&j2se-1_4;JavaUtilLoggingClassLibrary"/>
		<rdfs:comment xml:lang="en">JavaLibrary implementing the java.util.logging package for J2SE 5.0</rdfs:comment>
		<rdfs:comment xml:lang="OWLManchester">platform:implementsInterface some JavaUtilLoggingAPI</rdfs:comment>
	</owl:Class>
	<owl:Class rdf:about="&j2se-5_0;JavaUtilPrefsClassLibrary">
		<owl:equivalentClass rdf:resource="&j2se-1_4;JavaUtilPrefsClassLibrary"/>
		<rdfs:subClassOf rdf:resource="&java;JavaClassLibrary"/>
		<rdfs:comment xml:lang="en">JavaLibrary implementing the java.util.prefs package for J2SE 5.0</rdfs:comment>
		<rdfs:comment xml:lang="OWLManchester">platform:implementsInterface some JavaUtilPrefsAPI</rdfs:comment>
	</owl:Class>
	<owl:Class rdf:about="&j2se-5_0;JavaAppletClassLibrary">
		<rdfs:subClassOf rdf:resource="&j2se-1_4;JavaAppletClassLibrary"/>
		<rdfs:comment xml:lang="en">JavaLibrary implementing the java.applet package for J2SE 5.0</rdfs:comment>
		<rdfs:comment xml:lang="OWLManchester">platform:implementsInterface some JavaAppletAPI</rdfs:comment>
	</owl:Class>
	<owl:Class rdf:about="&j2se-5_0;JavaAwtClassLibrary">
		<rdfs:subClassOf rdf:resource="&j2se-1_4;JavaAwtClassLibrary"/>
		<rdfs:comment xml:lang="en">JavaLibrary implementing the java.awt package for J2SE 5.0</rdfs:comment>
		<rdfs:comment xml:lang="OWLManchester">platform:implementsInterface some JavaAwtAPI</rdfs:comment>
	</owl:Class>
	<owl:Class rdf:about="&j2se-5_0;JavaAwtEventClassLibrary">
		<rdfs:subClassOf rdf:resource="&j2se-1_4;JavaAwtEventClassLibrary"/>
		<rdfs:comment xml:lang="en">JavaLibrary implementing the java.awt.event package for J2SE 5.0</rdfs:comment>
		<rdfs:comment xml:lang="OWLManchester">platform:implementsInterface some JavaAwtEventAPI</rdfs:comment>
	</owl:Class>
	<owl:Class rdf:about="&j2se-5_0;JavaAwtImageClassLibrary">
		<rdfs:subClassOf rdf:resource="&j2se-1_4;JavaAwtImageClassLibrary"/>
		<rdfs:comment xml:lang="en">JavaLibrary implementing the java.awt.image package for J2SE 5.0</rdfs:comment>
		<rdfs:comment xml:lang="OWLManchester">platform:implementsInterface some JavaAwtImageAPI</rdfs:comment>
	</owl:Class>
	<owl:Class rdf:about="&j2se-5_0;JavaAwtImageRenderableClassLibrary">
		<owl:equivalentClass rdf:resource="&j2se-1_4;JavaAwtImageRenderableClassLibrary"/>
		<rdfs:subClassOf rdf:resource="&java;JavaClassLibrary"/>
		<rdfs:comment xml:lang="en">JavaLibrary implementing the java.awt.image.renderable package for J2SE 5.0</rdfs:comment>
		<rdfs:comment xml:lang="OWLManchester">platform:implementsInterface some JavaAwtImageRenderableAPI</rdfs:comment>
	</owl:Class>
	<owl:Class rdf:about="&j2se-5_0;JavaAwtGeomClassLibrary">
		<owl:equivalentClass rdf:resource="&j2se-1_4;JavaAwtGeomClassLibrary"/>
		<rdfs:subClassOf rdf:resource="&java;JavaClassLibrary"/>
		<rdfs:comment xml:lang="en">JavaLibrary implementing the java.awt.geom package for J2SE 5.0</rdfs:comment>
		<rdfs:comment xml:lang="OWLManchester">platform:implementsInterface some JavaAwtGeomAPI</rdfs:comment>
	</owl:Class>
	<owl:Class rdf:about="&j2se-5_0;JavaAwtImClassLibrary">
		<owl:equivalentClass rdf:resource="&j2se-1_4;JavaAwtImClassLibrary"/>
		<rdfs:subClassOf rdf:resource="&java;JavaClassLibrary"/>
		<rdfs:comment xml:lang="en">JavaLibrary implementing the java.awt.im package for J2SE 5.0</rdfs:comment>
		<rdfs:comment xml:lang="OWLManchester">platform:implementsInterface some JavaAwtImAPI</rdfs:comment>
	</owl:Class>
	<owl:Class rdf:about="&j2se-5_0;JavaAwtImSpiClassLibrary">
		<owl:equivalentClass rdf:resource="&j2se-1_4;JavaAwtImSpiClassLibrary"/>
		<rdfs:subClassOf rdf:resource="&java;JavaClassLibrary"/>
		<rdfs:comment xml:lang="en">JavaLibrary implementing the java.awt.im.spi package for J2SE 5.0</rdfs:comment>
		<rdfs:comment xml:lang="OWLManchester">platform:implementsInterface some JavaAwtImSpiAPI</rdfs:comment>
	</owl:Class>
	<owl:Class rdf:about="&j2se-5_0;JavaAwtColorClassLibrary">
		<rdfs:subClassOf rdf:resource="&j2se-1_4;JavaAwtColorClassLibrary"/>
		<rdfs:comment xml:lang="en">JavaLibrary implementing the java.awt.color package for J2SE 5.0</rdfs:comment>
		<rdfs:comment xml:lang="OWLManchester">platform:implementsInterface some JavaAwtColorAPI</rdfs:comment>
	</owl:Class>
	<owl:Class rdf:about="&j2se-5_0;JavaAwtDatatransferClassLibrary">
		<rdfs:subClassOf rdf:resource="&j2se-1_4;JavaAwtDatatransferClassLibrary"/>
		<rdfs:comment xml:lang="en">JavaLibrary implementing the java.awt.datatransfer package for J2SE 5.0</rdfs:comment>
		<rdfs:comment xml:lang="OWLManchester">platform:implementsInterface some JavaAwtDatatransferAPI</rdfs:comment>
	</owl:Class>
	<owl:Class rdf:about="&j2se-5_0;JavaAwtDndClassLibrary">
		<rdfs:subClassOf rdf:resource="&j2se-1_4;JavaAwtDndClassLibrary"/>
		<rdfs:comment xml:lang="en">JavaLibrary implementing the java.awt.dnd package for J2SE 5.0</rdfs:comment>
		<rdfs:comment xml:lang="OWLManchester">platform:implementsInterface some JavaAwtDndAPI</rdfs:comment>
	</owl:Class>
	<owl:Class rdf:about="&j2se-5_0;JavaAwtFontClassLibrary">
		<owl:equivalentClass rdf:resource="&j2se-1_4;JavaAwtFontClassLibrary"/>
		<rdfs:subClassOf rdf:resource="&java;JavaClassLibrary"/>
		<rdfs:comment xml:lang="en">JavaLibrary implementing the java.awt.font package for J2SE 5.0</rdfs:comment>
		<rdfs:comment xml:lang="OWLManchester">platform:implementsInterface some JavaAwtFontAPI</rdfs:comment>
	</owl:Class>
	<owl:Class rdf:about="&j2se-5_0;JavaAwtPrintClassLibrary">
		<owl:equivalentClass rdf:resource="&j2se-1_4;JavaAwtPrintClassLibrary"/>
		<rdfs:subClassOf rdf:resource="&java;JavaClassLibrary"/>
		<rdfs:comment xml:lang="en">JavaLibrary implementing the java.awt.print package for J2SE 5.0</rdfs:comment>
		<rdfs:comment xml:lang="OWLManchester">platform:implementsInterface some JavaAwtPrintAPI</rdfs:comment>
	</owl:Class>
	<owl:Class rdf:about="&j2se-5_0;JavaTextClassLibrary">
		<rdfs:subClassOf rdf:resource="&j2se-1_4;JavaTextClassLibrary"/>
		<rdfs:comment xml:lang="en">JavaLibrary implementing the java.text package for J2SE 5.0</rdfs:comment>
		<rdfs:comment xml:lang="OWLManchester">platform:implementsInterface some JavaTextAPI</rdfs:comment>
	</owl:Class>
	<owl:Class rdf:about="&j2se-5_0;JavaBeansClassLibrary">
		<rdfs:subClassOf rdf:resource="&j2se-1_4;JavaBeansClassLibrary"/>
		<rdfs:comment xml:lang="en">JavaLibrary implementing the java.beans package for J2SE 5.0</rdfs:comment>
		<rdfs:comment xml:lang="OWLManchester">platform:implementsInterface some JavaBeansAPI</rdfs:comment>
	</owl:Class>
	<owl:Class rdf:about="&j2se-5_0;JavaBeansBeancontextClassLibrary">
		<owl:equivalentClass rdf:resource="&j2se-1_4;JavaBeansBeancontextClassLibrary"/>
		<rdfs:subClassOf rdf:resource="&java;JavaClassLibrary"/>
		<rdfs:comment xml:lang="en">JavaLibrary implementing the java.beans.beancontext package for J2SE 5.0</rdfs:comment>
		<rdfs:comment xml:lang="OWLManchester">platform:implementsInterface some JavaBeansBeancontextAPI</rdfs:comment>
	</owl:Class>
	<owl:Class rdf:about="&j2se-5_0;JavaRmiClassLibrary">
		<owl:equivalentClass rdf:resource="&j2se-1_4;JavaRmiClassLibrary"/>
		<rdfs:subClassOf rdf:resource="&java;JavaClassLibrary"/>
		<rdfs:comment xml:lang="en">JavaLibrary implementing the java.rmi package for J2SE 5.0</rdfs:comment>
		<rdfs:comment xml:lang="OWLManchester">platform:implementsInterface some JavaRmiAPI</rdfs:comment>
	</owl:Class>
	<owl:Class rdf:about="&j2se-5_0;JavaRmiActivationClassLibrary">
		<owl:equivalentClass rdf:resource="&j2se-1_4;JavaRmiActivationClassLibrary"/>
		<rdfs:subClassOf rdf:resource="&java;JavaClassLibrary"/>
		<rdfs:comment xml:lang="en">JavaLibrary implementing the java.rmi.activation package for J2SE 5.0</rdfs:comment>
		<rdfs:comment xml:lang="OWLManchester">platform:implementsInterface some JavaRmiActivationAPI</rdfs:comment>
	</owl:Class>
	<owl:Class rdf:about="&j2se-5_0;JavaRmiServerClassLibrary">
		<rdfs:subClassOf rdf:resource="&j2se-1_4;JavaRmiServerClassLibrary"/>
		<rdfs:comment xml:lang="en">JavaLibrary implementing the java.rmi.server package for J2SE 5.0</rdfs:comment>
		<rdfs:comment xml:lang="OWLManchester">platform:implementsInterface some JavaRmiServerAPI</rdfs:comment>
	</owl:Class>
	<owl:Class rdf:about="&j2se-5_0;JavaRmiDgcClassLibrary">
		<owl:equivalentClass rdf:resource="&j2se-1_4;JavaRmiDgcClassLibrary"/>
		<rdfs:subClassOf rdf:resource="&java;JavaClassLibrary"/>
		<rdfs:comment xml:lang="en">JavaLibrary implementing the java.rmi.dgc package for J2SE 5.0</rdfs:comment>
		<rdfs:comment xml:lang="OWLManchester">platform:implementsInterface some JavaRmiDgcAPI</rdfs:comment>
	</owl:Class>
	<owl:Class rdf:about="&j2se-5_0;JavaRmiRegistryClassLibrary">
		<owl:equivalentClass rdf:resource="&j2se-1_4;JavaRmiRegistryClassLibrary"/>
		<rdfs:subClassOf rdf:resource="&java;JavaClassLibrary"/>
		<rdfs:comment xml:lang="en">JavaLibrary implementing the java.rmi.registry package for J2SE 5.0</rdfs:comment>
		<rdfs:comment xml:lang="OWLManchester">platform:implementsInterface some JavaRmiRegistryAPI</rdfs:comment>
	</owl:Class>
	<owl:Class rdf:about="&j2se-5_0;JavaSqlClassLibrary">
		<owl:equivalentClass rdf:resource="&j2se-1_4;JavaSqlClassLibrary"/>
		<rdfs:subClassOf rdf:resource="&java;JavaClassLibrary"/>
		<rdfs:comment xml:lang="en">JavaLibrary implementing the java.sql package for J2SE 5.0</rdfs:comment>
		<rdfs:comment xml:lang="OWLManchester">platform:implementsInterface some JavaSqlAPI</rdfs:comment>
	</owl:Class>
	<owl:Class rdf:about="&j2se-5_0;OrgW3cDomClassLibrary">
		<rdfs:subClassOf rdf:resource="&j2se-1_4;OrgW3cDomClassLibrary"/>
		<rdfs:comment xml:lang="en">JavaLibrary implementing the org.w3c.dom package for J2SE 5.0</rdfs:comment>
		<rdfs:comment xml:lang="OWLManchester">platform:implementsInterface some OrgW3cDomAPI</rdfs:comment>
	</owl:Class>
	<owl:Class rdf:about="&j2se-5_0;OrgW3cDomLsClassLibrary">
		<rdfs:subClassOf rdf:resource="&java;JavaClassLibrary"/>
		<rdfs:comment xml:lang="en">JavaLibrary implementing the org.w3c.dom.ls package for J2SE 5.0</rdfs:comment>
		<rdfs:comment xml:lang="OWLManchester">platform:implementsInterface some OrgW3cDomLsAPI</rdfs:comment>
	</owl:Class>
	<owl:Class rdf:about="&j2se-5_0;OrgW3cDomBootstrapClassLibrary">
		<rdfs:subClassOf rdf:resource="&java;JavaClassLibrary"/>
		<rdfs:comment xml:lang="en">JavaLibrary implementing the org.w3c.dom.bootstrap package for J2SE 5.0</rdfs:comment>
		<rdfs:comment xml:lang="OWLManchester">platform:implementsInterface some OrgW3cDomBootstrapAPI</rdfs:comment>
	</owl:Class>
	<owl:Class rdf:about="&j2se-5_0;OrgW3cDomCssClassLibrary">
		<rdfs:subClassOf rdf:resource="&j2se-1_4;OrgW3cDomCssClassLibrary"/>
		<rdfs:comment xml:lang="en">JavaLibrary implementing the org.w3c.dom.css package for J2SE 5.0</rdfs:comment>
		<rdfs:comment xml:lang="OWLManchester">platform:implementsInterface some OrgW3cDomCssAPI</rdfs:comment>
	</owl:Class>
	<owl:Class rdf:about="&j2se-5_0;OrgW3cDomStylesheetsClassLibrary">
		<owl:equivalentClass rdf:resource="&j2se-1_4;OrgW3cDomStylesheetsClassLibrary"/>
		<rdfs:subClassOf rdf:resource="&java;JavaClassLibrary"/>
		<rdfs:comment xml:lang="en">JavaLibrary implementing the org.w3c.dom.stylesheets package for J2SE 5.0</rdfs:comment>
		<rdfs:comment xml:lang="OWLManchester">platform:implementsInterface some OrgW3cDomStylesheetsAPI</rdfs:comment>
	</owl:Class>
	<owl:Class rdf:about="&j2se-5_0;OrgW3cDomViewsClassLibrary">
		<owl:equivalentClass rdf:resource="&j2se-1_4;OrgW3cDomViewsClassLibrary"/>
		<rdfs:subClassOf rdf:resource="&java;JavaClassLibrary"/>
		<rdfs:comment xml:lang="en">JavaLibrary implementing the org.w3c.dom.views package for J2SE 5.0</rdfs:comment>
		<rdfs:comment xml:lang="OWLManchester">platform:implementsInterface some OrgW3cDomViewsAPI</rdfs:comment>
	</owl:Class>
	<owl:Class rdf:about="&j2se-5_0;OrgW3cDomEventsClassLibrary">
		<owl:equivalentClass rdf:resource="&j2se-1_4;OrgW3cDomEventsClassLibrary"/>
		<rdfs:subClassOf rdf:resource="&java;JavaClassLibrary"/>
		<rdfs:comment xml:lang="en">JavaLibrary implementing the org.w3c.dom.events package for J2SE 5.0</rdfs:comment>
		<rdfs:comment xml:lang="OWLManchester">platform:implementsInterface some OrgW3cDomEventsAPI</rdfs:comment>
	</owl:Class>
	<owl:Class rdf:about="&j2se-5_0;OrgW3cDomHtmlClassLibrary">
		<rdfs:subClassOf rdf:resource="&j2se-1_4;OrgW3cDomHtmlClassLibrary"/>
		<rdfs:comment xml:lang="en">JavaLibrary implementing the org.w3c.dom.html package for J2SE 5.0</rdfs:comment>
		<rdfs:comment xml:lang="OWLManchester">platform:implementsInterface some OrgW3cDomHtmlAPI</rdfs:comment>
	</owl:Class>
	<owl:Class rdf:about="&j2se-5_0;OrgW3cDomTraversalClassLibrary">
		<owl:equivalentClass rdf:resource="&j2se-1_4;OrgW3cDomTraversalClassLibrary"/>
		<rdfs:subClassOf rdf:resource="&java;JavaClassLibrary"/>
		<rdfs:comment xml:lang="en">JavaLibrary implementing the org.w3c.dom.traversal package for J2SE 5.0</rdfs:comment>
		<rdfs:comment xml:lang="OWLManchester">platform:implementsInterface some OrgW3cDomTraversalAPI</rdfs:comment>
	</owl:Class>
	<owl:Class rdf:about="&j2se-5_0;OrgW3cDomRangesClassLibrary">
		<rdfs:subClassOf rdf:resource="&java;JavaClassLibrary"/>
		<rdfs:comment xml:lang="en">JavaLibrary implementing the org.w3c.dom.ranges package for J2SE 5.0</rdfs:comment>
		<rdfs:comment xml:lang="OWLManchester">platform:implementsInterface some OrgW3cDomRangesAPI</rdfs:comment>
	</owl:Class>
	<owl:Class rdf:about="&j2se-5_0;OrgOmgCORBA_2_3ClassLibrary">
		<owl:equivalentClass rdf:resource="&j2se-1_4;OrgOmgCORBA_2_3ClassLibrary"/>
		<rdfs:subClassOf rdf:resource="&java;JavaClassLibrary"/>
		<rdfs:comment xml:lang="en">JavaLibrary implementing the org.omg.CORBA_2_3 package for J2SE 5.0</rdfs:comment>
		<rdfs:comment xml:lang="OWLManchester">platform:implementsInterface some OrgOmgCORBA_2_3API</rdfs:comment>
	</owl:Class>
	<owl:Class rdf:about="&j2se-5_0;OrgOmgCORBA_2_3PortableClassLibrary">
		<owl:equivalentClass rdf:resource="&j2se-1_4;OrgOmgCORBA_2_3PortableClassLibrary"/>
		<rdfs:subClassOf rdf:resource="&java;JavaClassLibrary"/>
		<rdfs:comment xml:lang="en">JavaLibrary implementing the org.omg.CORBA_2_3.portable package for J2SE 5.0</rdfs:comment>
		<rdfs:comment xml:lang="OWLManchester">platform:implementsInterface some OrgOmgCORBA_2_3PortableAPI</rdfs:comment>
	</owl:Class>
	<owl:Class rdf:about="&j2se-5_0;OrgOmgCORBAClassLibrary">
		<rdfs:subClassOf rdf:resource="&j2se-1_4;OrgOmgCORBAClassLibrary"/>
		<rdfs:comment xml:lang="en">JavaLibrary implementing the org.omg.CORBA package for J2SE 5.0</rdfs:comment>
		<rdfs:comment xml:lang="OWLManchester">platform:implementsInterface some OrgOmgCORBAAPI</rdfs:comment>
	</owl:Class>
	<owl:Class rdf:about="&j2se-5_0;OrgOmgCORBAPortableClassLibrary">
		<rdfs:subClassOf rdf:resource="&j2se-1_4;OrgOmgCORBAPortableClassLibrary"/>
		<rdfs:comment xml:lang="en">JavaLibrary implementing the org.omg.CORBA.portable package for J2SE 5.0</rdfs:comment>
		<rdfs:comment xml:lang="OWLManchester">platform:implementsInterface some OrgOmgCORBAPortableAPI</rdfs:comment>
	</owl:Class>
	<owl:Class rdf:about="&j2se-5_0;OrgOmgCORBADynAnyPackageClassLibrary">
		<owl:equivalentClass rdf:resource="&j2se-1_4;OrgOmgCORBADynAnyPackageClassLibrary"/>
		<rdfs:subClassOf rdf:resource="&java;JavaClassLibrary"/>
		<rdfs:comment xml:lang="en">JavaLibrary implementing the org.omg.CORBA.DynAnyPackage package for J2SE 5.0</rdfs:comment>
		<rdfs:comment xml:lang="OWLManchester">platform:implementsInterface some OrgOmgCORBADynAnyPackageAPI</rdfs:comment>
	</owl:Class>
	<owl:Class rdf:about="&j2se-5_0;OrgOmgCORBAORBPackageClassLibrary">
		<owl:equivalentClass rdf:resource="&j2se-1_4;OrgOmgCORBAORBPackageClassLibrary"/>
		<rdfs:subClassOf rdf:resource="&java;JavaClassLibrary"/>
		<rdfs:comment xml:lang="en">JavaLibrary implementing the org.omg.CORBA.ORBPackage package for J2SE 5.0</rdfs:comment>
		<rdfs:comment xml:lang="OWLManchester">platform:implementsInterface some OrgOmgCORBAORBPackageAPI</rdfs:comment>
	</owl:Class>
	<owl:Class rdf:about="&j2se-5_0;OrgOmgCORBATypeCodePackageClassLibrary">
		<owl:equivalentClass rdf:resource="&j2se-1_4;OrgOmgCORBATypeCodePackageClassLibrary"/>
		<rdfs:subClassOf rdf:resource="&java;JavaClassLibrary"/>
		<rdfs:comment xml:lang="en">JavaLibrary implementing the org.omg.CORBA.TypeCodePackage package for J2SE 5.0</rdfs:comment>
		<rdfs:comment xml:lang="OWLManchester">platform:implementsInterface some OrgOmgCORBATypeCodePackageAPI</rdfs:comment>
	</owl:Class>
	<owl:Class rdf:about="&j2se-5_0;OrgOmgSendingContextClassLibrary">
		<owl:equivalentClass rdf:resource="&j2se-1_4;OrgOmgSendingContextClassLibrary"/>
		<rdfs:subClassOf rdf:resource="&java;JavaClassLibrary"/>
		<rdfs:comment xml:lang="en">JavaLibrary implementing the org.omg.SendingContext package for J2SE 5.0</rdfs:comment>
		<rdfs:comment xml:lang="OWLManchester">platform:implementsInterface some OrgOmgSendingContextAPI</rdfs:comment>
	</owl:Class>
	<owl:Class rdf:about="&j2se-5_0;OrgOmgCosNamingClassLibrary">
		<rdfs:subClassOf rdf:resource="&j2se-1_4;OrgOmgCosNamingClassLibrary"/>
		<rdfs:comment xml:lang="en">JavaLibrary implementing the org.omg.CosNaming package for J2SE 5.0</rdfs:comment>
		<rdfs:comment xml:lang="OWLManchester">platform:implementsInterface some OrgOmgCosNamingAPI</rdfs:comment>
	</owl:Class>
	<owl:Class rdf:about="&j2se-5_0;OrgOmgCosNamingNamingContextExtPackageClassLibrary">
		<owl:equivalentClass rdf:resource="&j2se-1_4;OrgOmgCosNamingNamingContextExtPackageClassLibrary"/>
		<rdfs:subClassOf rdf:resource="&java;JavaClassLibrary"/>
		<rdfs:comment xml:lang="en">JavaLibrary implementing the org.omg.CosNaming.NamingContextExtPackage package for J2SE 5.0</rdfs:comment>
		<rdfs:comment xml:lang="OWLManchester">platform:implementsInterface some OrgOmgCosNamingNamingContextExtPackageAPI</rdfs:comment>
	</owl:Class>
	<owl:Class rdf:about="&j2se-5_0;OrgOmgCosNamingNamingContextPackageClassLibrary">
		<owl:equivalentClass rdf:resource="&j2se-1_4;OrgOmgCosNamingNamingContextPackageClassLibrary"/>
		<rdfs:subClassOf rdf:resource="&java;JavaClassLibrary"/>
		<rdfs:comment xml:lang="en">JavaLibrary implementing the org.omg.CosNaming.NamingContextPackage package for J2SE 5.0</rdfs:comment>
		<rdfs:comment xml:lang="OWLManchester">platform:implementsInterface some OrgOmgCosNamingNamingContextPackageAPI</rdfs:comment>
	</owl:Class>
	<owl:Class rdf:about="&j2se-5_0;OrgOmgPortableServerClassLibrary">
		<rdfs:subClassOf rdf:resource="&j2se-1_4;OrgOmgPortableServerClassLibrary"/>
		<rdfs:comment xml:lang="en">JavaLibrary implementing the org.omg.PortableServer package for J2SE 5.0</rdfs:comment>
		<rdfs:comment xml:lang="OWLManchester">platform:implementsInterface some OrgOmgPortableServerAPI</rdfs:comment>
	</owl:Class>
	<owl:Class rdf:about="&j2se-5_0;OrgOmgPortableServerCurrentPackageClassLibrary">
		<owl:equivalentClass rdf:resource="&j2se-1_4;OrgOmgPortableServerCurrentPackageClassLibrary"/>
		<rdfs:subClassOf rdf:resource="&java;JavaClassLibrary"/>
		<rdfs:comment xml:lang="en">JavaLibrary implementing the org.omg.PortableServer.CurrentPackage package for J2SE 5.0</rdfs:comment>
		<rdfs:comment xml:lang="OWLManchester">platform:implementsInterface some OrgOmgPortableServerCurrentPackageAPI</rdfs:comment>
	</owl:Class>
	<owl:Class rdf:about="&j2se-5_0;OrgOmgPortableServerPOAManagerPackageClassLibrary">
		<owl:equivalentClass rdf:resource="&j2se-1_4;OrgOmgPortableServerPOAManagerPackageClassLibrary"/>
		<rdfs:subClassOf rdf:resource="&java;JavaClassLibrary"/>
		<rdfs:comment xml:lang="en">JavaLibrary implementing the org.omg.PortableServer.POAManagerPackage package for J2SE 5.0</rdfs:comment>
		<rdfs:comment xml:lang="OWLManchester">platform:implementsInterface some OrgOmgPortableServerPOAManagerPackageAPI</rdfs:comment>
	</owl:Class>
	<owl:Class rdf:about="&j2se-5_0;OrgOmgPortableServerPOAPackageClassLibrary">
		<owl:equivalentClass rdf:resource="&j2se-1_4;OrgOmgPortableServerPOAPackageClassLibrary"/>
		<rdfs:subClassOf rdf:resource="&java;JavaClassLibrary"/>
		<rdfs:comment xml:lang="en">JavaLibrary implementing the org.omg.PortableServer.POAPackage package for J2SE 5.0</rdfs:comment>
		<rdfs:comment xml:lang="OWLManchester">platform:implementsInterface some OrgOmgPortableServerPOAPackageAPI</rdfs:comment>
	</owl:Class>
	<owl:Class rdf:about="&j2se-5_0;OrgOmgPortableServerPortableClassLibrary">
		<owl:equivalentClass rdf:resource="&j2se-1_4;OrgOmgPortableServerPortableClassLibrary"/>
		<rdfs:subClassOf rdf:resource="&java;JavaClassLibrary"/>
		<rdfs:comment xml:lang="en">JavaLibrary implementing the org.omg.PortableServer.portable package for J2SE 5.0</rdfs:comment>
		<rdfs:comment xml:lang="OWLManchester">platform:implementsInterface some OrgOmgPortableServerPortableAPI</rdfs:comment>
	</owl:Class>
	<owl:Class rdf:about="&j2se-5_0;OrgOmgPortableServerServantLocatorPackageClassLibrary">
		<owl:equivalentClass rdf:resource="&j2se-1_4;OrgOmgPortableServerServantLocatorPackageClassLibrary"/>
		<rdfs:subClassOf rdf:resource="&java;JavaClassLibrary"/>
		<rdfs:comment xml:lang="en">JavaLibrary implementing the org.omg.PortableServer.ServantLocatorPackage package for J2SE 5.0</rdfs:comment>
		<rdfs:comment xml:lang="OWLManchester">platform:implementsInterface some OrgOmgPortableServerServantLocatorPackageAPI</rdfs:comment>
	</owl:Class>
	<owl:Class rdf:about="&j2se-5_0;OrgOmgDynamicClassLibrary">
		<owl:equivalentClass rdf:resource="&j2se-1_4;OrgOmgDynamicClassLibrary"/>
		<rdfs:subClassOf rdf:resource="&java;JavaClassLibrary"/>
		<rdfs:comment xml:lang="en">JavaLibrary implementing the org.omg.Dynamic package for J2SE 5.0</rdfs:comment>
		<rdfs:comment xml:lang="OWLManchester">platform:implementsInterface some OrgOmgDynamicAPI</rdfs:comment>
	</owl:Class>
	<owl:Class rdf:about="&j2se-5_0;OrgOmgDynamicAnyClassLibrary">
		<rdfs:subClassOf rdf:resource="&j2se-1_4;OrgOmgDynamicAnyClassLibrary"/>
		<rdfs:comment xml:lang="en">JavaLibrary implementing the org.omg.DynamicAny package for J2SE 5.0</rdfs:comment>
		<rdfs:comment xml:lang="OWLManchester">platform:implementsInterface some OrgOmgDynamicAnyAPI</rdfs:comment>
	</owl:Class>
	<owl:Class rdf:about="&j2se-5_0;OrgOmgDynamicAnyDynAnyFactoryPackageClassLibrary">
		<owl:equivalentClass rdf:resource="&j2se-1_4;OrgOmgDynamicAnyDynAnyFactoryPackageClassLibrary"/>
		<rdfs:subClassOf rdf:resource="&java;JavaClassLibrary"/>
		<rdfs:comment xml:lang="en">JavaLibrary implementing the org.omg.DynamicAny.DynAnyFactoryPackage package for J2SE 5.0</rdfs:comment>
		<rdfs:comment xml:lang="OWLManchester">platform:implementsInterface some OrgOmgDynamicAnyDynAnyFactoryPackageAPI</rdfs:comment>
	</owl:Class>
	<owl:Class rdf:about="&j2se-5_0;OrgOmgDynamicAnyDynAnyPackageClassLibrary">
		<owl:equivalentClass rdf:resource="&j2se-1_4;OrgOmgDynamicAnyDynAnyPackageClassLibrary"/>
		<rdfs:subClassOf rdf:resource="&java;JavaClassLibrary"/>
		<rdfs:comment xml:lang="en">JavaLibrary implementing the org.omg.DynamicAny.DynAnyPackage package for J2SE 5.0</rdfs:comment>
		<rdfs:comment xml:lang="OWLManchester">platform:implementsInterface some OrgOmgDynamicAnyDynAnyPackageAPI</rdfs:comment>
	</owl:Class>
	<owl:Class rdf:about="&j2se-5_0;OrgOmgIOPClassLibrary">
		<rdfs:subClassOf rdf:resource="&j2se-1_4;OrgOmgIOPClassLibrary"/>
		<rdfs:comment xml:lang="en">JavaLibrary implementing the org.omg.IOP package for J2SE 5.0</rdfs:comment>
		<rdfs:comment xml:lang="OWLManchester">platform:implementsInterface some OrgOmgIOPAPI</rdfs:comment>
	</owl:Class>
	<owl:Class rdf:about="&j2se-5_0;OrgOmgIOPCodecFactoryPackageClassLibrary">
		<owl:equivalentClass rdf:resource="&j2se-1_4;OrgOmgIOPCodecFactoryPackageClassLibrary"/>
		<rdfs:subClassOf rdf:resource="&java;JavaClassLibrary"/>
		<rdfs:comment xml:lang="en">JavaLibrary implementing the org.omg.IOP.CodecFactoryPackage package for J2SE 5.0</rdfs:comment>
		<rdfs:comment xml:lang="OWLManchester">platform:implementsInterface some OrgOmgIOPCodecFactoryPackageAPI</rdfs:comment>
	</owl:Class>
	<owl:Class rdf:about="&j2se-5_0;OrgOmgIOPCodecPackageClassLibrary">
		<owl:equivalentClass rdf:resource="&j2se-1_4;OrgOmgIOPCodecPackageClassLibrary"/>
		<rdfs:subClassOf rdf:resource="&java;JavaClassLibrary"/>
		<rdfs:comment xml:lang="en">JavaLibrary implementing the org.omg.IOP.CodecPackage package for J2SE 5.0</rdfs:comment>
		<rdfs:comment xml:lang="OWLManchester">platform:implementsInterface some OrgOmgIOPCodecPackageAPI</rdfs:comment>
	</owl:Class>
	<owl:Class rdf:about="&j2se-5_0;OrgOmgMessagingClassLibrary">
		<owl:equivalentClass rdf:resource="&j2se-1_4;OrgOmgMessagingClassLibrary"/>
		<rdfs:subClassOf rdf:resource="&java;JavaClassLibrary"/>
		<rdfs:comment xml:lang="en">JavaLibrary implementing the org.omg.Messaging package for J2SE 5.0</rdfs:comment>
		<rdfs:comment xml:lang="OWLManchester">platform:implementsInterface some OrgOmgMessagingAPI</rdfs:comment>
	</owl:Class>
	<owl:Class rdf:about="&j2se-5_0;OrgOmgPortableInterceptorClassLibrary">
		<rdfs:subClassOf rdf:resource="&j2se-1_4;OrgOmgPortableInterceptorClassLibrary"/>
		<rdfs:comment xml:lang="en">JavaLibrary implementing the org.omg.PortableInterceptor package for J2SE 5.0</rdfs:comment>
		<rdfs:comment xml:lang="OWLManchester">platform:implementsInterface some OrgOmgPortableInterceptorAPI</rdfs:comment>
	</owl:Class>
	<owl:Class rdf:about="&j2se-5_0;OrgOmgPortableInterceptorORBInitInfoPackageClassLibrary">
		<owl:equivalentClass rdf:resource="&j2se-1_4;OrgOmgPortableInterceptorORBInitInfoPackageClassLibrary"/>
		<rdfs:subClassOf rdf:resource="&java;JavaClassLibrary"/>
		<rdfs:comment xml:lang="en">JavaLibrary implementing the org.omg.PortableInterceptor.ORBInitInfoPackage package for J2SE 5.0</rdfs:comment>
		<rdfs:comment xml:lang="OWLManchester">platform:implementsInterface some OrgOmgPortableInterceptorORBInitInfoPackageAPI</rdfs:comment>
	</owl:Class>
	<owl:Class rdf:about="&j2se-5_0;OrgOmgStubJavaRmiClassLibrary">
		<owl:equivalentClass rdf:resource="&j2se-1_4;OrgOmgStubJavaRmiClassLibrary"/>
		<rdfs:subClassOf rdf:resource="&java;JavaClassLibrary"/>
		<rdfs:comment xml:lang="en">JavaLibrary implementing the org.omg.stub.java.rmi package for J2SE 5.0</rdfs:comment>
		<rdfs:comment xml:lang="OWLManchester">platform:implementsInterface some OrgOmgStubJavaRmiAPI</rdfs:comment>
	</owl:Class>
	<owl:Class rdf:about="&j2se-5_0;OrgOmgStubJavaxManagementRemoteRmiClassLibrary">
		<rdfs:subClassOf rdf:resource="&java;JavaClassLibrary"/>
		<rdfs:comment xml:lang="en">JavaLibrary implementing the org.omg.stub.javax.management.remote.rmi package for J2SE 5.0</rdfs:comment>
		<rdfs:comment xml:lang="OWLManchester">platform:implementsInterface some OrgOmgStubJavaxManagementRemoteRmiAPI</rdfs:comment>
	</owl:Class>
	<owl:Class rdf:about="&j2se-5_0;OrgXmlSaxClassLibrary">
		<owl:equivalentClass rdf:resource="&j2se-1_4;OrgXmlSaxClassLibrary"/>
		<rdfs:subClassOf rdf:resource="&java;JavaClassLibrary"/>
		<rdfs:comment xml:lang="en">JavaLibrary implementing the org.xml.sax package for J2SE 5.0</rdfs:comment>
		<rdfs:comment xml:lang="OWLManchester">platform:implementsInterface some OrgXmlSaxAPI</rdfs:comment>
	</owl:Class>
	<owl:Class rdf:about="&j2se-5_0;OrgXmlSaxExtClassLibrary">
		<rdfs:subClassOf rdf:resource="&j2se-1_4;OrgXmlSaxExtClassLibrary"/>
		<rdfs:comment xml:lang="en">JavaLibrary implementing the org.xml.sax.ext package for J2SE 5.0</rdfs:comment>
		<rdfs:comment xml:lang="OWLManchester">platform:implementsInterface some OrgXmlSaxExtAPI</rdfs:comment>
	</owl:Class>
	<owl:Class rdf:about="&j2se-5_0;OrgXmlSaxHelpersClassLibrary">
		<rdfs:subClassOf rdf:resource="&j2se-1_4;OrgXmlSaxHelpersClassLibrary"/>
		<rdfs:comment xml:lang="en">JavaLibrary implementing the org.xml.sax.helpers package for J2SE 5.0</rdfs:comment>
		<rdfs:comment xml:lang="OWLManchester">platform:implementsInterface some OrgXmlSaxHelpersAPI</rdfs:comment>
	</owl:Class>
	<owl:Class rdf:about="&j2se-5_0;OrgIetfJgssClassLibrary">
		<owl:equivalentClass rdf:resource="&j2se-1_4;OrgIetfJgssClassLibrary"/>
		<rdfs:subClassOf rdf:resource="&java;JavaClassLibrary"/>
		<rdfs:comment xml:lang="en">JavaLibrary implementing the org.ietf.jgss package for J2SE 5.0</rdfs:comment>
		<rdfs:comment xml:lang="OWLManchester">platform:implementsInterface some OrgIetfJgssAPI</rdfs:comment>
	</owl:Class>
</rdf:RDF>
