<?xml version="1.0" encoding="ISO-8859-1"?>
<!DOCTYPE rdf:RDF [
	<!ENTITY isa "http://localhost/~dennis/platformkit/2010_1/isa.owl#">
	<!ENTITY platform "http://localhost/~dennis/platformkit/2010_1/platform.owl#">
	<!ENTITY swt-3_0 "http://soft.vub.ac.be/platformkit/2010/1/swt-3_0.owl#">
	<!ENTITY java "http://localhost/~dennis/platformkit/2010_1/java.owl#">
	<!ENTITY xsd "http://www.w3.org/2001/XMLSchema#">
	<!ENTITY rdf "http://www.w3.org/1999/02/22-rdf-syntax-ns#">
	<!ENTITY owl "http://www.w3.org/2002/07/owl#">
	<!ENTITY ns_3 "http://localhost/~dennis/platformkit/2010_1/">
	<!ENTITY rdfs "http://www.w3.org/2000/01/rdf-schema#">
]>
<rdf:RDF
	 xmlns:isa="&isa;"
	 xmlns:platform="&platform;"
	 xmlns:swt-3_0="&swt-3_0;"
	 xmlns:java="&java;"
	 xmlns:xsd="&xsd;"
	 xmlns:rdf="&rdf;"
	 xmlns:owl="&owl;"
	 xmlns:ns_3="&ns_3;"
	 xmlns:rdfs="&rdfs;"
>

	<owl:Ontology rdf:about="http://soft.vub.ac.be/platformkit/2010/1/swt-3_0.owl#">
		<owl:versionInfo>$Id: UML2ToPackageAPIOntology.atl 8082 2010-03-18 21:11:00Z dwagelaa $</owl:versionInfo>
		<owl:imports rdf:resource="http://localhost/~dennis/platformkit/2010_1/platform.owl"/>
		<owl:imports rdf:resource="http://localhost/~dennis/platformkit/2010_1/java.owl"/>
		<rdfs:comment xml:lang="en">Generated by [UML2ToSimplifiedPackageAPIOntology.atl 8080 2010-03-18 10:46:40Z dwagelaa], [UML2ToPackageAPIOntology.atl 8082 2010-03-18 21:11:00Z dwagelaa], [UML2ToAPIOntology.atl 8086 2010-03-19 09:49:17Z dwagelaa], and [UML2Comparison.atl 8086 2010-03-19 09:49:17Z dwagelaa]</rdfs:comment>
		<rdfs:comment>Dennis Wagelaar &lt;dennis.wagelaar@vub.ac.be&gt;</rdfs:comment>
		<rdfs:comment xml:lang="en">&#169; 2010, Vrije Universiteit Brussel. All rights reserved.</rdfs:comment>
		<rdfs:label xml:lang="en">SWT 3.0</rdfs:label>
	</owl:Ontology>
	<owl:Class rdf:about="&swt-3_0;SWT3_0API">
		<rdfs:subClassOf rdf:resource="&swt-3_0;OrgEclipseSwtAPI"/>
		<rdfs:subClassOf rdf:resource="&swt-3_0;OrgEclipseSwtAccessibilityAPI"/>
		<rdfs:subClassOf rdf:resource="&swt-3_0;OrgEclipseSwtWidgetsAPI"/>
		<rdfs:subClassOf rdf:resource="&swt-3_0;OrgEclipseSwtAwtAPI"/>
		<rdfs:subClassOf rdf:resource="&swt-3_0;OrgEclipseSwtBrowserAPI"/>
		<rdfs:subClassOf rdf:resource="&swt-3_0;OrgEclipseSwtEventsAPI"/>
		<rdfs:subClassOf rdf:resource="&swt-3_0;OrgEclipseSwtGraphicsAPI"/>
		<rdfs:subClassOf rdf:resource="&swt-3_0;OrgEclipseSwtCustomAPI"/>
		<rdfs:subClassOf rdf:resource="&swt-3_0;OrgEclipseSwtPrintingAPI"/>
		<rdfs:subClassOf rdf:resource="&swt-3_0;OrgEclipseSwtDndAPI"/>
		<rdfs:subClassOf rdf:resource="&swt-3_0;OrgEclipseSwtLayoutAPI"/>
		<rdfs:subClassOf rdf:resource="&swt-3_0;OrgEclipseSwtProgramAPI"/>
		<rdfs:comment xml:lang="en">SWT 3.0 API</rdfs:comment>
		<rdfs:comment xml:lang="OWLManchester">platform:comprisesInterfacePart some OrgEclipseSwt and platform:comprisesInterfacePart some OrgEclipseSwtAccessibility and platform:comprisesInterfacePart some OrgEclipseSwtWidgets and platform:comprisesInterfacePart some OrgEclipseSwtAwt and platform:comprisesInterfacePart some OrgEclipseSwtBrowser and platform:comprisesInterfacePart some OrgEclipseSwtEvents and platform:comprisesInterfacePart some OrgEclipseSwtGraphics and platform:comprisesInterfacePart some OrgEclipseSwtCustom and platform:comprisesInterfacePart some OrgEclipseSwtPrinting and platform:comprisesInterfacePart some OrgEclipseSwtDnd and platform:comprisesInterfacePart some OrgEclipseSwtLayout and platform:comprisesInterfacePart some OrgEclipseSwtProgram</rdfs:comment>
	</owl:Class>
	<owl:Class rdf:about="&swt-3_0;SWT3_0ClassLibrary">
		<rdfs:subClassOf rdf:resource="&swt-3_0;OrgEclipseSwtClassLibrary"/>
		<rdfs:subClassOf rdf:resource="&swt-3_0;OrgEclipseSwtAccessibilityClassLibrary"/>
		<rdfs:subClassOf rdf:resource="&swt-3_0;OrgEclipseSwtWidgetsClassLibrary"/>
		<rdfs:subClassOf rdf:resource="&swt-3_0;OrgEclipseSwtAwtClassLibrary"/>
		<rdfs:subClassOf rdf:resource="&swt-3_0;OrgEclipseSwtBrowserClassLibrary"/>
		<rdfs:subClassOf rdf:resource="&swt-3_0;OrgEclipseSwtEventsClassLibrary"/>
		<rdfs:subClassOf rdf:resource="&swt-3_0;OrgEclipseSwtGraphicsClassLibrary"/>
		<rdfs:subClassOf rdf:resource="&swt-3_0;OrgEclipseSwtCustomClassLibrary"/>
		<rdfs:subClassOf rdf:resource="&swt-3_0;OrgEclipseSwtPrintingClassLibrary"/>
		<rdfs:subClassOf rdf:resource="&swt-3_0;OrgEclipseSwtDndClassLibrary"/>
		<rdfs:subClassOf rdf:resource="&swt-3_0;OrgEclipseSwtLayoutClassLibrary"/>
		<rdfs:subClassOf rdf:resource="&swt-3_0;OrgEclipseSwtProgramClassLibrary"/>
		<rdfs:comment xml:lang="en">Java class library implementing the SWT 3.0 API</rdfs:comment>
		<rdfs:comment xml:lang="OWLManchester">platform:implementsInterface some SWT3_0API</rdfs:comment>
	</owl:Class>
	<owl:Class rdf:about="&swt-3_0;SWT3_0BytecodeFormat">
		<rdfs:subClassOf rdf:resource="&isa;JavaBytecode"/>
		<rdfs:comment xml:lang="en">SWT 3.0 bytecode format</rdfs:comment>
		<rdfs:comment xml:lang="OWLManchester">java:majorVersionNumber some xsd:integer[>="46"^^xsd:integer] and java:preverified value false</rdfs:comment>
	</owl:Class>
	<swt-3_0:SWT3_0BytecodeFormat rdf:about="&swt-3_0;theSWT3_0BytecodeFormat">
		<java:preverified rdf:datatype="http://www.w3.org/2001/XMLSchema#boolean">false</java:preverified>
		<java:minorVersionNumber rdf:datatype="http://www.w3.org/2001/XMLSchema#integer">0</java:minorVersionNumber>
		<java:majorVersionNumber rdf:datatype="http://www.w3.org/2001/XMLSchema#integer">46</java:majorVersionNumber>
	</swt-3_0:SWT3_0BytecodeFormat>
	<swt-3_0:SWT3_0API rdf:about="&swt-3_0;theSWT3_0API">
		<platform:comprisesInterfacePart rdf:resource="&swt-3_0;theOrgEclipseSwtProgramPart"/>
		<platform:comprisesInterfacePart rdf:resource="&swt-3_0;theOrgEclipseSwtLayoutPart"/>
		<platform:comprisesInterfacePart rdf:resource="&swt-3_0;theOrgEclipseSwtDndPart"/>
		<platform:comprisesInterfacePart rdf:resource="&swt-3_0;theOrgEclipseSwtPrintingPart"/>
		<platform:comprisesInterfacePart rdf:resource="&swt-3_0;theOrgEclipseSwtCustomPart"/>
		<platform:comprisesInterfacePart rdf:resource="&swt-3_0;theOrgEclipseSwtGraphicsPart"/>
		<platform:comprisesInterfacePart rdf:resource="&swt-3_0;theOrgEclipseSwtEventsPart"/>
		<platform:comprisesInterfacePart rdf:resource="&swt-3_0;theOrgEclipseSwtBrowserPart"/>
		<platform:comprisesInterfacePart rdf:resource="&swt-3_0;theOrgEclipseSwtAwtPart"/>
		<platform:comprisesInterfacePart rdf:resource="&swt-3_0;theOrgEclipseSwtWidgetsPart"/>
		<platform:comprisesInterfacePart rdf:resource="&swt-3_0;theOrgEclipseSwtAccessibilityPart"/>
		<platform:comprisesInterfacePart rdf:resource="&swt-3_0;theOrgEclipseSwtPart"/>
	</swt-3_0:SWT3_0API>
	<owl:Class rdf:about="&swt-3_0;SWT3_0VM">
		<owl:equivalentClass>
			<owl:Restriction>
				<owl:onProperty rdf:resource="&platform;implementsInterface"/>
				<owl:someValuesFrom rdf:resource="&swt-3_0;SWT3_0BytecodeFormat"/>
			</owl:Restriction>
		</owl:equivalentClass>
		<rdfs:subClassOf rdf:resource="&java;JavaVM"/>
		<rdfs:comment xml:lang="en">SWT 3.0 virtual machine</rdfs:comment>
	</owl:Class>
	<owl:Class rdf:about="&swt-3_0;SWT3_0JRE">
		<owl:equivalentClass>
			<owl:Class >
				<owl:intersectionOf rdf:parseType="Collection">
					<owl:Restriction>
						<owl:onProperty rdf:resource="&platform;providesFeature"/>
						<owl:someValuesFrom rdf:resource="&swt-3_0;SWT3_0ClassLibrary"/>
					</owl:Restriction>
					<owl:Restriction>
						<owl:onProperty rdf:resource="&platform;providesFeature"/>
						<owl:someValuesFrom rdf:resource="&swt-3_0;SWT3_0VM"/>
					</owl:Restriction>
				</owl:intersectionOf>
			</owl:Class>
		</owl:equivalentClass>
		<rdfs:subClassOf rdf:resource="&java;JRE"/>
		<rdfs:comment xml:lang="en">SWT 3.0 Java Runtime Environment</rdfs:comment>
	</owl:Class>
	<owl:Class rdf:about="&swt-3_0;OrgEclipseSwt">
		<rdfs:subClassOf rdf:resource="&java;JavaAPIPart"/>
		<rdfs:comment xml:lang="en">Java API part implementing the org.eclipse.swt package for SWT 3.0</rdfs:comment>
	</owl:Class>
	<owl:Class rdf:about="&swt-3_0;OrgEclipseSwtAccessibility">
		<rdfs:subClassOf rdf:resource="&java;JavaAPIPart"/>
		<rdfs:seeAlso rdf:resource="&swt-3_0;OrgEclipseSwtWidgets"/>
		<rdfs:comment xml:lang="en">Java API part implementing the org.eclipse.swt.accessibility package for SWT 3.0</rdfs:comment>
	</owl:Class>
	<owl:Class rdf:about="&swt-3_0;OrgEclipseSwtWidgets">
		<rdfs:subClassOf rdf:resource="&java;JavaAPIPart"/>
		<rdfs:seeAlso rdf:resource="&swt-3_0;OrgEclipseSwtAccessibility"/>
		<rdfs:seeAlso rdf:resource="&swt-3_0;OrgEclipseSwtGraphics"/>
		<rdfs:seeAlso rdf:resource="&swt-3_0;OrgEclipseSwtEvents"/>
		<rdfs:comment xml:lang="en">Java API part implementing the org.eclipse.swt.widgets package for SWT 3.0</rdfs:comment>
	</owl:Class>
	<owl:Class rdf:about="&swt-3_0;OrgEclipseSwtAwt">
		<rdfs:subClassOf rdf:resource="&java;JavaAPIPart"/>
		<rdfs:seeAlso rdf:resource="&swt-3_0;OrgEclipseSwtWidgets"/>
		<rdfs:comment xml:lang="en">Java API part implementing the org.eclipse.swt.awt package for SWT 3.0</rdfs:comment>
	</owl:Class>
	<owl:Class rdf:about="&swt-3_0;OrgEclipseSwtBrowser">
		<rdfs:subClassOf rdf:resource="&java;JavaAPIPart"/>
		<rdfs:seeAlso rdf:resource="&swt-3_0;OrgEclipseSwtWidgets"/>
		<rdfs:seeAlso rdf:resource="&swt-3_0;OrgEclipseSwtGraphics"/>
		<rdfs:seeAlso rdf:resource="&swt-3_0;OrgEclipseSwtEvents"/>
		<rdfs:comment xml:lang="en">Java API part implementing the org.eclipse.swt.browser package for SWT 3.0</rdfs:comment>
	</owl:Class>
	<owl:Class rdf:about="&swt-3_0;OrgEclipseSwtEvents">
		<rdfs:subClassOf rdf:resource="&java;JavaAPIPart"/>
		<rdfs:seeAlso rdf:resource="&swt-3_0;OrgEclipseSwtWidgets"/>
		<rdfs:seeAlso rdf:resource="&swt-3_0;OrgEclipseSwtGraphics"/>
		<rdfs:comment xml:lang="en">Java API part implementing the org.eclipse.swt.events package for SWT 3.0</rdfs:comment>
	</owl:Class>
	<owl:Class rdf:about="&swt-3_0;OrgEclipseSwtGraphics">
		<rdfs:subClassOf rdf:resource="&java;JavaAPIPart"/>
		<rdfs:comment xml:lang="en">Java API part implementing the org.eclipse.swt.graphics package for SWT 3.0</rdfs:comment>
	</owl:Class>
	<owl:Class rdf:about="&swt-3_0;OrgEclipseSwtCustom">
		<rdfs:subClassOf rdf:resource="&java;JavaAPIPart"/>
		<rdfs:seeAlso rdf:resource="&swt-3_0;OrgEclipseSwtGraphics"/>
		<rdfs:seeAlso rdf:resource="&swt-3_0;OrgEclipseSwtPrinting"/>
		<rdfs:seeAlso rdf:resource="&swt-3_0;OrgEclipseSwtEvents"/>
		<rdfs:seeAlso rdf:resource="&swt-3_0;OrgEclipseSwtWidgets"/>
		<rdfs:comment xml:lang="en">Java API part implementing the org.eclipse.swt.custom package for SWT 3.0</rdfs:comment>
	</owl:Class>
	<owl:Class rdf:about="&swt-3_0;OrgEclipseSwtPrinting">
		<rdfs:subClassOf rdf:resource="&java;JavaAPIPart"/>
		<rdfs:seeAlso rdf:resource="&swt-3_0;OrgEclipseSwtWidgets"/>
		<rdfs:seeAlso rdf:resource="&swt-3_0;OrgEclipseSwtGraphics"/>
		<rdfs:comment xml:lang="en">Java API part implementing the org.eclipse.swt.printing package for SWT 3.0</rdfs:comment>
	</owl:Class>
	<owl:Class rdf:about="&swt-3_0;OrgEclipseSwtDnd">
		<rdfs:subClassOf rdf:resource="&java;JavaAPIPart"/>
		<rdfs:seeAlso rdf:resource="&swt-3_0;OrgEclipseSwtWidgets"/>
		<rdfs:seeAlso rdf:resource="&swt-3_0;OrgEclipseSwtEvents"/>
		<rdfs:comment xml:lang="en">Java API part implementing the org.eclipse.swt.dnd package for SWT 3.0</rdfs:comment>
	</owl:Class>
	<owl:Class rdf:about="&swt-3_0;OrgEclipseSwtLayout">
		<rdfs:subClassOf rdf:resource="&java;JavaAPIPart"/>
		<rdfs:seeAlso rdf:resource="&swt-3_0;OrgEclipseSwtGraphics"/>
		<rdfs:seeAlso rdf:resource="&swt-3_0;OrgEclipseSwtWidgets"/>
		<rdfs:comment xml:lang="en">Java API part implementing the org.eclipse.swt.layout package for SWT 3.0</rdfs:comment>
	</owl:Class>
	<owl:Class rdf:about="&swt-3_0;OrgEclipseSwtProgram">
		<rdfs:subClassOf rdf:resource="&java;JavaAPIPart"/>
		<rdfs:seeAlso rdf:resource="&swt-3_0;OrgEclipseSwtGraphics"/>
		<rdfs:comment xml:lang="en">Java API part implementing the org.eclipse.swt.program package for SWT 3.0</rdfs:comment>
	</owl:Class>
	<owl:Class rdf:about="&swt-3_0;OrgEclipseSwtAPI">
		<rdfs:subClassOf rdf:resource="&java;JavaAPI"/>
		<rdfs:comment xml:lang="en">JavaLibrary implementing the org.eclipse.swt package for SWT 3.0</rdfs:comment>
		<rdfs:comment xml:lang="OWLManchester">platform:comprisesInterfacePart some OrgEclipseSwt</rdfs:comment>
	</owl:Class>
	<owl:Class rdf:about="&swt-3_0;OrgEclipseSwtAccessibilityAPI">
		<rdfs:subClassOf rdf:resource="&java;JavaAPI"/>
		<rdfs:comment xml:lang="en">JavaLibrary implementing the org.eclipse.swt.accessibility package for SWT 3.0</rdfs:comment>
		<rdfs:comment xml:lang="OWLManchester">platform:comprisesInterfacePart some OrgEclipseSwtAccessibility</rdfs:comment>
	</owl:Class>
	<owl:Class rdf:about="&swt-3_0;OrgEclipseSwtWidgetsAPI">
		<rdfs:subClassOf rdf:resource="&java;JavaAPI"/>
		<rdfs:comment xml:lang="en">JavaLibrary implementing the org.eclipse.swt.widgets package for SWT 3.0</rdfs:comment>
		<rdfs:comment xml:lang="OWLManchester">platform:comprisesInterfacePart some OrgEclipseSwtWidgets</rdfs:comment>
	</owl:Class>
	<owl:Class rdf:about="&swt-3_0;OrgEclipseSwtAwtAPI">
		<rdfs:subClassOf rdf:resource="&java;JavaAPI"/>
		<rdfs:comment xml:lang="en">JavaLibrary implementing the org.eclipse.swt.awt package for SWT 3.0</rdfs:comment>
		<rdfs:comment xml:lang="OWLManchester">platform:comprisesInterfacePart some OrgEclipseSwtAwt</rdfs:comment>
	</owl:Class>
	<owl:Class rdf:about="&swt-3_0;OrgEclipseSwtBrowserAPI">
		<rdfs:subClassOf rdf:resource="&java;JavaAPI"/>
		<rdfs:comment xml:lang="en">JavaLibrary implementing the org.eclipse.swt.browser package for SWT 3.0</rdfs:comment>
		<rdfs:comment xml:lang="OWLManchester">platform:comprisesInterfacePart some OrgEclipseSwtBrowser</rdfs:comment>
	</owl:Class>
	<owl:Class rdf:about="&swt-3_0;OrgEclipseSwtEventsAPI">
		<rdfs:subClassOf rdf:resource="&java;JavaAPI"/>
		<rdfs:comment xml:lang="en">JavaLibrary implementing the org.eclipse.swt.events package for SWT 3.0</rdfs:comment>
		<rdfs:comment xml:lang="OWLManchester">platform:comprisesInterfacePart some OrgEclipseSwtEvents</rdfs:comment>
	</owl:Class>
	<owl:Class rdf:about="&swt-3_0;OrgEclipseSwtGraphicsAPI">
		<rdfs:subClassOf rdf:resource="&java;JavaAPI"/>
		<rdfs:comment xml:lang="en">JavaLibrary implementing the org.eclipse.swt.graphics package for SWT 3.0</rdfs:comment>
		<rdfs:comment xml:lang="OWLManchester">platform:comprisesInterfacePart some OrgEclipseSwtGraphics</rdfs:comment>
	</owl:Class>
	<owl:Class rdf:about="&swt-3_0;OrgEclipseSwtCustomAPI">
		<rdfs:subClassOf rdf:resource="&java;JavaAPI"/>
		<rdfs:comment xml:lang="en">JavaLibrary implementing the org.eclipse.swt.custom package for SWT 3.0</rdfs:comment>
		<rdfs:comment xml:lang="OWLManchester">platform:comprisesInterfacePart some OrgEclipseSwtCustom</rdfs:comment>
	</owl:Class>
	<owl:Class rdf:about="&swt-3_0;OrgEclipseSwtPrintingAPI">
		<rdfs:subClassOf rdf:resource="&java;JavaAPI"/>
		<rdfs:comment xml:lang="en">JavaLibrary implementing the org.eclipse.swt.printing package for SWT 3.0</rdfs:comment>
		<rdfs:comment xml:lang="OWLManchester">platform:comprisesInterfacePart some OrgEclipseSwtPrinting</rdfs:comment>
	</owl:Class>
	<owl:Class rdf:about="&swt-3_0;OrgEclipseSwtDndAPI">
		<rdfs:subClassOf rdf:resource="&java;JavaAPI"/>
		<rdfs:comment xml:lang="en">JavaLibrary implementing the org.eclipse.swt.dnd package for SWT 3.0</rdfs:comment>
		<rdfs:comment xml:lang="OWLManchester">platform:comprisesInterfacePart some OrgEclipseSwtDnd</rdfs:comment>
	</owl:Class>
	<owl:Class rdf:about="&swt-3_0;OrgEclipseSwtLayoutAPI">
		<rdfs:subClassOf rdf:resource="&java;JavaAPI"/>
		<rdfs:comment xml:lang="en">JavaLibrary implementing the org.eclipse.swt.layout package for SWT 3.0</rdfs:comment>
		<rdfs:comment xml:lang="OWLManchester">platform:comprisesInterfacePart some OrgEclipseSwtLayout</rdfs:comment>
	</owl:Class>
	<owl:Class rdf:about="&swt-3_0;OrgEclipseSwtProgramAPI">
		<rdfs:subClassOf rdf:resource="&java;JavaAPI"/>
		<rdfs:comment xml:lang="en">JavaLibrary implementing the org.eclipse.swt.program package for SWT 3.0</rdfs:comment>
		<rdfs:comment xml:lang="OWLManchester">platform:comprisesInterfacePart some OrgEclipseSwtProgram</rdfs:comment>
	</owl:Class>
	<swt-3_0:OrgEclipseSwt rdf:about="&swt-3_0;theOrgEclipseSwtPart">
	</swt-3_0:OrgEclipseSwt>
	<swt-3_0:OrgEclipseSwtAccessibility rdf:about="&swt-3_0;theOrgEclipseSwtAccessibilityPart">
	</swt-3_0:OrgEclipseSwtAccessibility>
	<swt-3_0:OrgEclipseSwtWidgets rdf:about="&swt-3_0;theOrgEclipseSwtWidgetsPart">
	</swt-3_0:OrgEclipseSwtWidgets>
	<swt-3_0:OrgEclipseSwtAwt rdf:about="&swt-3_0;theOrgEclipseSwtAwtPart">
	</swt-3_0:OrgEclipseSwtAwt>
	<swt-3_0:OrgEclipseSwtBrowser rdf:about="&swt-3_0;theOrgEclipseSwtBrowserPart">
	</swt-3_0:OrgEclipseSwtBrowser>
	<swt-3_0:OrgEclipseSwtEvents rdf:about="&swt-3_0;theOrgEclipseSwtEventsPart">
	</swt-3_0:OrgEclipseSwtEvents>
	<swt-3_0:OrgEclipseSwtGraphics rdf:about="&swt-3_0;theOrgEclipseSwtGraphicsPart">
	</swt-3_0:OrgEclipseSwtGraphics>
	<swt-3_0:OrgEclipseSwtCustom rdf:about="&swt-3_0;theOrgEclipseSwtCustomPart">
	</swt-3_0:OrgEclipseSwtCustom>
	<swt-3_0:OrgEclipseSwtPrinting rdf:about="&swt-3_0;theOrgEclipseSwtPrintingPart">
	</swt-3_0:OrgEclipseSwtPrinting>
	<swt-3_0:OrgEclipseSwtDnd rdf:about="&swt-3_0;theOrgEclipseSwtDndPart">
	</swt-3_0:OrgEclipseSwtDnd>
	<swt-3_0:OrgEclipseSwtLayout rdf:about="&swt-3_0;theOrgEclipseSwtLayoutPart">
	</swt-3_0:OrgEclipseSwtLayout>
	<swt-3_0:OrgEclipseSwtProgram rdf:about="&swt-3_0;theOrgEclipseSwtProgramPart">
	</swt-3_0:OrgEclipseSwtProgram>
	<owl:Class rdf:about="&swt-3_0;OrgEclipseSwtClassLibrary">
		<rdfs:subClassOf rdf:resource="&java;JavaClassLibrary"/>
		<rdfs:comment xml:lang="en">JavaLibrary implementing the org.eclipse.swt package for SWT 3.0</rdfs:comment>
		<rdfs:comment xml:lang="OWLManchester">platform:implementsInterface some OrgEclipseSwtAPI</rdfs:comment>
	</owl:Class>
	<owl:Class rdf:about="&swt-3_0;OrgEclipseSwtAccessibilityClassLibrary">
		<rdfs:subClassOf rdf:resource="&java;JavaClassLibrary"/>
		<rdfs:comment xml:lang="en">JavaLibrary implementing the org.eclipse.swt.accessibility package for SWT 3.0</rdfs:comment>
		<rdfs:comment xml:lang="OWLManchester">platform:implementsInterface some OrgEclipseSwtAccessibilityAPI</rdfs:comment>
	</owl:Class>
	<owl:Class rdf:about="&swt-3_0;OrgEclipseSwtWidgetsClassLibrary">
		<rdfs:subClassOf rdf:resource="&java;JavaClassLibrary"/>
		<rdfs:comment xml:lang="en">JavaLibrary implementing the org.eclipse.swt.widgets package for SWT 3.0</rdfs:comment>
		<rdfs:comment xml:lang="OWLManchester">platform:implementsInterface some OrgEclipseSwtWidgetsAPI</rdfs:comment>
	</owl:Class>
	<owl:Class rdf:about="&swt-3_0;OrgEclipseSwtAwtClassLibrary">
		<rdfs:subClassOf rdf:resource="&java;JavaClassLibrary"/>
		<rdfs:comment xml:lang="en">JavaLibrary implementing the org.eclipse.swt.awt package for SWT 3.0</rdfs:comment>
		<rdfs:comment xml:lang="OWLManchester">platform:implementsInterface some OrgEclipseSwtAwtAPI</rdfs:comment>
	</owl:Class>
	<owl:Class rdf:about="&swt-3_0;OrgEclipseSwtBrowserClassLibrary">
		<rdfs:subClassOf rdf:resource="&java;JavaClassLibrary"/>
		<rdfs:comment xml:lang="en">JavaLibrary implementing the org.eclipse.swt.browser package for SWT 3.0</rdfs:comment>
		<rdfs:comment xml:lang="OWLManchester">platform:implementsInterface some OrgEclipseSwtBrowserAPI</rdfs:comment>
	</owl:Class>
	<owl:Class rdf:about="&swt-3_0;OrgEclipseSwtEventsClassLibrary">
		<rdfs:subClassOf rdf:resource="&java;JavaClassLibrary"/>
		<rdfs:comment xml:lang="en">JavaLibrary implementing the org.eclipse.swt.events package for SWT 3.0</rdfs:comment>
		<rdfs:comment xml:lang="OWLManchester">platform:implementsInterface some OrgEclipseSwtEventsAPI</rdfs:comment>
	</owl:Class>
	<owl:Class rdf:about="&swt-3_0;OrgEclipseSwtGraphicsClassLibrary">
		<rdfs:subClassOf rdf:resource="&java;JavaClassLibrary"/>
		<rdfs:comment xml:lang="en">JavaLibrary implementing the org.eclipse.swt.graphics package for SWT 3.0</rdfs:comment>
		<rdfs:comment xml:lang="OWLManchester">platform:implementsInterface some OrgEclipseSwtGraphicsAPI</rdfs:comment>
	</owl:Class>
	<owl:Class rdf:about="&swt-3_0;OrgEclipseSwtCustomClassLibrary">
		<rdfs:subClassOf rdf:resource="&java;JavaClassLibrary"/>
		<rdfs:comment xml:lang="en">JavaLibrary implementing the org.eclipse.swt.custom package for SWT 3.0</rdfs:comment>
		<rdfs:comment xml:lang="OWLManchester">platform:implementsInterface some OrgEclipseSwtCustomAPI</rdfs:comment>
	</owl:Class>
	<owl:Class rdf:about="&swt-3_0;OrgEclipseSwtPrintingClassLibrary">
		<rdfs:subClassOf rdf:resource="&java;JavaClassLibrary"/>
		<rdfs:comment xml:lang="en">JavaLibrary implementing the org.eclipse.swt.printing package for SWT 3.0</rdfs:comment>
		<rdfs:comment xml:lang="OWLManchester">platform:implementsInterface some OrgEclipseSwtPrintingAPI</rdfs:comment>
	</owl:Class>
	<owl:Class rdf:about="&swt-3_0;OrgEclipseSwtDndClassLibrary">
		<rdfs:subClassOf rdf:resource="&java;JavaClassLibrary"/>
		<rdfs:comment xml:lang="en">JavaLibrary implementing the org.eclipse.swt.dnd package for SWT 3.0</rdfs:comment>
		<rdfs:comment xml:lang="OWLManchester">platform:implementsInterface some OrgEclipseSwtDndAPI</rdfs:comment>
	</owl:Class>
	<owl:Class rdf:about="&swt-3_0;OrgEclipseSwtLayoutClassLibrary">
		<rdfs:subClassOf rdf:resource="&java;JavaClassLibrary"/>
		<rdfs:comment xml:lang="en">JavaLibrary implementing the org.eclipse.swt.layout package for SWT 3.0</rdfs:comment>
		<rdfs:comment xml:lang="OWLManchester">platform:implementsInterface some OrgEclipseSwtLayoutAPI</rdfs:comment>
	</owl:Class>
	<owl:Class rdf:about="&swt-3_0;OrgEclipseSwtProgramClassLibrary">
		<rdfs:subClassOf rdf:resource="&java;JavaClassLibrary"/>
		<rdfs:comment xml:lang="en">JavaLibrary implementing the org.eclipse.swt.program package for SWT 3.0</rdfs:comment>
		<rdfs:comment xml:lang="OWLManchester">platform:implementsInterface some OrgEclipseSwtProgramAPI</rdfs:comment>
	</owl:Class>
</rdf:RDF>
