<?xml version="1.0" encoding="ISO-8859-1"?>
<!DOCTYPE rdf:RDF [
	<!ENTITY isa "http://localhost/~dennis/platformkit/2010_1/isa.owl#">
	<!ENTITY xsd "http://www.w3.org/2001/XMLSchema#">
	<!ENTITY swt-3_3 "http://soft.vub.ac.be/platformkit/2010/1/swt-3_3.owl#">
	<!ENTITY java "http://localhost/~dennis/platformkit/2010_1/java.owl#">
	<!ENTITY swt-3_2 "http://soft.vub.ac.be/platformkit/2010/1/swt-3_2.owl#">
	<!ENTITY ns_5 "http://localhost/~dennis/platformkit/2010_1/">
	<!ENTITY platform "http://localhost/~dennis/platformkit/2010_1/platform.owl#">
	<!ENTITY rdfs "http://www.w3.org/2000/01/rdf-schema#">
	<!ENTITY rdf "http://www.w3.org/1999/02/22-rdf-syntax-ns#">
	<!ENTITY owl "http://www.w3.org/2002/07/owl#">
]>
<rdf:RDF
	 xmlns:isa="&isa;"
	 xmlns:xsd="&xsd;"
	 xmlns:swt-3_3="&swt-3_3;"
	 xmlns:java="&java;"
	 xmlns:swt-3_2="&swt-3_2;"
	 xmlns:ns_5="&ns_5;"
	 xmlns:platform="&platform;"
	 xmlns:rdfs="&rdfs;"
	 xmlns:rdf="&rdf;"
	 xmlns:owl="&owl;"
>

	<owl:Ontology rdf:about="http://soft.vub.ac.be/platformkit/2010/1/swt-3_3.owl#">
		<owl:versionInfo>$Id: UML2ToPackageAPIOntology.atl 8082 2010-03-18 21:11:00Z dwagelaa $</owl:versionInfo>
		<owl:imports rdf:resource="http://localhost/~dennis/platformkit/2010_1/platform.owl"/>
		<owl:imports rdf:resource="http://localhost/~dennis/platformkit/2010_1/java.owl"/>
		<owl:imports rdf:resource="http://soft.vub.ac.be/platformkit/2010/1/swt-3_2.owl#"/>
		<owl:imports rdf:resource="http://localhost/~dennis/platformkit/2010_1/isa.owl"/>
		<rdfs:comment xml:lang="en">Generated by [UML2ToSimplifiedPackageAPIOntology.atl 8080 2010-03-18 10:46:40Z dwagelaa], [UML2ToPackageAPIOntology.atl 8082 2010-03-18 21:11:00Z dwagelaa], [UML2ToAPIOntology.atl 8086 2010-03-19 09:49:17Z dwagelaa], and [UML2Comparison.atl 8086 2010-03-19 09:49:17Z dwagelaa]</rdfs:comment>
		<rdfs:comment>Dennis Wagelaar &lt;dennis.wagelaar@vub.ac.be&gt;</rdfs:comment>
		<rdfs:comment xml:lang="en">&#169; 2010, Vrije Universiteit Brussel. All rights reserved.</rdfs:comment>
		<rdfs:label xml:lang="en">SWT 3.3</rdfs:label>
	</owl:Ontology>
	<owl:Class rdf:about="&swt-3_3;SWT3_3API">
		<rdfs:subClassOf rdf:resource="&swt-3_3;OrgEclipseSwtAPI"/>
		<rdfs:subClassOf rdf:resource="&swt-3_3;OrgEclipseSwtAccessibilityAPI"/>
		<rdfs:subClassOf rdf:resource="&swt-3_3;OrgEclipseSwtWidgetsAPI"/>
		<rdfs:subClassOf rdf:resource="&swt-3_3;OrgEclipseSwtAwtAPI"/>
		<rdfs:subClassOf rdf:resource="&swt-3_3;OrgEclipseSwtBrowserAPI"/>
		<rdfs:subClassOf rdf:resource="&swt-3_3;OrgEclipseSwtEventsAPI"/>
		<rdfs:subClassOf rdf:resource="&swt-3_3;OrgEclipseSwtGraphicsAPI"/>
		<rdfs:subClassOf rdf:resource="&swt-3_3;OrgEclipseSwtCustomAPI"/>
		<rdfs:subClassOf rdf:resource="&swt-3_3;OrgEclipseSwtPrintingAPI"/>
		<rdfs:subClassOf rdf:resource="&swt-3_3;OrgEclipseSwtDndAPI"/>
		<rdfs:subClassOf rdf:resource="&swt-3_3;OrgEclipseSwtLayoutAPI"/>
		<rdfs:subClassOf rdf:resource="&swt-3_3;OrgEclipseSwtOpenglAPI"/>
		<rdfs:subClassOf rdf:resource="&swt-3_3;OrgEclipseSwtProgramAPI"/>
		<rdfs:subClassOf rdf:resource="&swt-3_2;SWT3_2API"/>
		<rdfs:comment xml:lang="en">SWT 3.3 API</rdfs:comment>
		<rdfs:comment xml:lang="OWLManchester">platform:comprisesInterfacePart some OrgEclipseSwt and platform:comprisesInterfacePart some OrgEclipseSwtAccessibility and platform:comprisesInterfacePart some OrgEclipseSwtWidgets and platform:comprisesInterfacePart some OrgEclipseSwtAwt and platform:comprisesInterfacePart some OrgEclipseSwtBrowser and platform:comprisesInterfacePart some OrgEclipseSwtEvents and platform:comprisesInterfacePart some OrgEclipseSwtGraphics and platform:comprisesInterfacePart some OrgEclipseSwtCustom and platform:comprisesInterfacePart some OrgEclipseSwtPrinting and platform:comprisesInterfacePart some OrgEclipseSwtDnd and platform:comprisesInterfacePart some OrgEclipseSwtLayout and platform:comprisesInterfacePart some OrgEclipseSwtOpengl and platform:comprisesInterfacePart some OrgEclipseSwtProgram</rdfs:comment>
	</owl:Class>
	<owl:Class rdf:about="&swt-3_3;SWT3_3ClassLibrary">
		<rdfs:subClassOf rdf:resource="&swt-3_3;OrgEclipseSwtClassLibrary"/>
		<rdfs:subClassOf rdf:resource="&swt-3_3;OrgEclipseSwtAccessibilityClassLibrary"/>
		<rdfs:subClassOf rdf:resource="&swt-3_3;OrgEclipseSwtWidgetsClassLibrary"/>
		<rdfs:subClassOf rdf:resource="&swt-3_3;OrgEclipseSwtAwtClassLibrary"/>
		<rdfs:subClassOf rdf:resource="&swt-3_3;OrgEclipseSwtBrowserClassLibrary"/>
		<rdfs:subClassOf rdf:resource="&swt-3_3;OrgEclipseSwtEventsClassLibrary"/>
		<rdfs:subClassOf rdf:resource="&swt-3_3;OrgEclipseSwtGraphicsClassLibrary"/>
		<rdfs:subClassOf rdf:resource="&swt-3_3;OrgEclipseSwtCustomClassLibrary"/>
		<rdfs:subClassOf rdf:resource="&swt-3_3;OrgEclipseSwtPrintingClassLibrary"/>
		<rdfs:subClassOf rdf:resource="&swt-3_3;OrgEclipseSwtDndClassLibrary"/>
		<rdfs:subClassOf rdf:resource="&swt-3_3;OrgEclipseSwtLayoutClassLibrary"/>
		<rdfs:subClassOf rdf:resource="&swt-3_3;OrgEclipseSwtOpenglClassLibrary"/>
		<rdfs:subClassOf rdf:resource="&swt-3_3;OrgEclipseSwtProgramClassLibrary"/>
		<rdfs:subClassOf rdf:resource="&swt-3_2;SWT3_2ClassLibrary"/>
		<rdfs:comment xml:lang="en">Java class library implementing the SWT 3.3 API</rdfs:comment>
		<rdfs:comment xml:lang="OWLManchester">platform:implementsInterface some SWT3_3API</rdfs:comment>
	</owl:Class>
	<owl:Class rdf:about="&swt-3_3;SWT3_3BytecodeFormat">
		<owl:equivalentClass rdf:resource="&swt-3_2;SWT3_2BytecodeFormat"/>
		<rdfs:subClassOf rdf:resource="&isa;JavaBytecode"/>
		<rdfs:comment xml:lang="en">SWT 3.3 bytecode format</rdfs:comment>
		<rdfs:comment xml:lang="OWLManchester">java:majorVersionNumber some xsd:integer[>="46"^^xsd:integer] and java:preverified value false</rdfs:comment>
	</owl:Class>
	<swt-3_3:SWT3_3BytecodeFormat rdf:about="&swt-3_3;theSWT3_3BytecodeFormat">
		<java:preverified rdf:datatype="http://www.w3.org/2001/XMLSchema#boolean">false</java:preverified>
		<java:minorVersionNumber rdf:datatype="http://www.w3.org/2001/XMLSchema#integer">0</java:minorVersionNumber>
		<java:majorVersionNumber rdf:datatype="http://www.w3.org/2001/XMLSchema#integer">46</java:majorVersionNumber>
	</swt-3_3:SWT3_3BytecodeFormat>
	<swt-3_3:SWT3_3API rdf:about="&swt-3_3;theSWT3_3API">
		<platform:comprisesInterfacePart rdf:resource="&swt-3_3;theOrgEclipseSwtProgramPart"/>
		<platform:comprisesInterfacePart rdf:resource="&swt-3_3;theOrgEclipseSwtOpenglPart"/>
		<platform:comprisesInterfacePart rdf:resource="&swt-3_3;theOrgEclipseSwtLayoutPart"/>
		<platform:comprisesInterfacePart rdf:resource="&swt-3_3;theOrgEclipseSwtDndPart"/>
		<platform:comprisesInterfacePart rdf:resource="&swt-3_3;theOrgEclipseSwtPrintingPart"/>
		<platform:comprisesInterfacePart rdf:resource="&swt-3_3;theOrgEclipseSwtCustomPart"/>
		<platform:comprisesInterfacePart rdf:resource="&swt-3_3;theOrgEclipseSwtGraphicsPart"/>
		<platform:comprisesInterfacePart rdf:resource="&swt-3_3;theOrgEclipseSwtEventsPart"/>
		<platform:comprisesInterfacePart rdf:resource="&swt-3_3;theOrgEclipseSwtBrowserPart"/>
		<platform:comprisesInterfacePart rdf:resource="&swt-3_3;theOrgEclipseSwtAwtPart"/>
		<platform:comprisesInterfacePart rdf:resource="&swt-3_3;theOrgEclipseSwtWidgetsPart"/>
		<platform:comprisesInterfacePart rdf:resource="&swt-3_3;theOrgEclipseSwtAccessibilityPart"/>
		<platform:comprisesInterfacePart rdf:resource="&swt-3_3;theOrgEclipseSwtPart"/>
	</swt-3_3:SWT3_3API>
	<owl:Class rdf:about="&swt-3_3;SWT3_3VM">
		<owl:equivalentClass>
			<owl:Restriction>
				<owl:onProperty rdf:resource="&platform;implementsInterface"/>
				<owl:someValuesFrom rdf:resource="&swt-3_3;SWT3_3BytecodeFormat"/>
			</owl:Restriction>
		</owl:equivalentClass>
		<rdfs:subClassOf rdf:resource="&java;JavaVM"/>
		<rdfs:comment xml:lang="en">SWT 3.3 virtual machine</rdfs:comment>
	</owl:Class>
	<owl:Class rdf:about="&swt-3_3;SWT3_3JRE">
		<owl:equivalentClass>
			<owl:Class >
				<owl:intersectionOf rdf:parseType="Collection">
					<owl:Restriction>
						<owl:onProperty rdf:resource="&platform;providesFeature"/>
						<owl:someValuesFrom rdf:resource="&swt-3_3;SWT3_3ClassLibrary"/>
					</owl:Restriction>
					<owl:Restriction>
						<owl:onProperty rdf:resource="&platform;providesFeature"/>
						<owl:someValuesFrom rdf:resource="&swt-3_3;SWT3_3VM"/>
					</owl:Restriction>
				</owl:intersectionOf>
			</owl:Class>
		</owl:equivalentClass>
		<rdfs:subClassOf rdf:resource="&java;JRE"/>
		<rdfs:comment xml:lang="en">SWT 3.3 Java Runtime Environment</rdfs:comment>
	</owl:Class>
	<owl:Class rdf:about="&swt-3_3;OrgEclipseSwt">
		<rdfs:subClassOf rdf:resource="&swt-3_2;OrgEclipseSwt"/>
		<rdfs:comment xml:lang="en">Java API part implementing the org.eclipse.swt package for SWT 3.3</rdfs:comment>
	</owl:Class>
	<owl:Class rdf:about="&swt-3_3;OrgEclipseSwtAccessibility">
		<owl:equivalentClass rdf:resource="&swt-3_2;OrgEclipseSwtAccessibility"/>
		<rdfs:subClassOf rdf:resource="&java;JavaAPIPart"/>
		<rdfs:seeAlso rdf:resource="&swt-3_3;OrgEclipseSwtWidgets"/>
		<rdfs:comment xml:lang="en">Java API part implementing the org.eclipse.swt.accessibility package for SWT 3.3</rdfs:comment>
	</owl:Class>
	<owl:Class rdf:about="&swt-3_3;OrgEclipseSwtWidgets">
		<rdfs:subClassOf rdf:resource="&swt-3_2;OrgEclipseSwtWidgets"/>
		<rdfs:seeAlso rdf:resource="&swt-3_3;OrgEclipseSwtEvents"/>
		<rdfs:seeAlso rdf:resource="&swt-3_3;OrgEclipseSwtAccessibility"/>
		<rdfs:seeAlso rdf:resource="&swt-3_3;OrgEclipseSwtGraphics"/>
		<rdfs:comment xml:lang="en">Java API part implementing the org.eclipse.swt.widgets package for SWT 3.3</rdfs:comment>
	</owl:Class>
	<owl:Class rdf:about="&swt-3_3;OrgEclipseSwtAwt">
		<owl:equivalentClass rdf:resource="&swt-3_2;OrgEclipseSwtAwt"/>
		<rdfs:subClassOf rdf:resource="&java;JavaAPIPart"/>
		<rdfs:seeAlso rdf:resource="&swt-3_3;OrgEclipseSwtWidgets"/>
		<rdfs:comment xml:lang="en">Java API part implementing the org.eclipse.swt.awt package for SWT 3.3</rdfs:comment>
	</owl:Class>
	<owl:Class rdf:about="&swt-3_3;OrgEclipseSwtBrowser">
		<rdfs:subClassOf rdf:resource="&swt-3_2;OrgEclipseSwtBrowser"/>
		<rdfs:seeAlso rdf:resource="&swt-3_3;OrgEclipseSwtEvents"/>
		<rdfs:seeAlso rdf:resource="&swt-3_3;OrgEclipseSwtWidgets"/>
		<rdfs:seeAlso rdf:resource="&swt-3_3;OrgEclipseSwtGraphics"/>
		<rdfs:comment xml:lang="en">Java API part implementing the org.eclipse.swt.browser package for SWT 3.3</rdfs:comment>
	</owl:Class>
	<owl:Class rdf:about="&swt-3_3;OrgEclipseSwtEvents">
		<rdfs:subClassOf rdf:resource="&swt-3_2;OrgEclipseSwtEvents"/>
		<rdfs:seeAlso rdf:resource="&swt-3_3;OrgEclipseSwtWidgets"/>
		<rdfs:seeAlso rdf:resource="&swt-3_3;OrgEclipseSwtGraphics"/>
		<rdfs:comment xml:lang="en">Java API part implementing the org.eclipse.swt.events package for SWT 3.3</rdfs:comment>
	</owl:Class>
	<owl:Class rdf:about="&swt-3_3;OrgEclipseSwtGraphics">
		<rdfs:subClassOf rdf:resource="&swt-3_2;OrgEclipseSwtGraphics"/>
		<rdfs:comment xml:lang="en">Java API part implementing the org.eclipse.swt.graphics package for SWT 3.3</rdfs:comment>
	</owl:Class>
	<owl:Class rdf:about="&swt-3_3;OrgEclipseSwtCustom">
		<rdfs:subClassOf rdf:resource="&swt-3_2;OrgEclipseSwtCustom"/>
		<rdfs:seeAlso rdf:resource="&swt-3_3;OrgEclipseSwtEvents"/>
		<rdfs:seeAlso rdf:resource="&swt-3_3;OrgEclipseSwtWidgets"/>
		<rdfs:seeAlso rdf:resource="&swt-3_3;OrgEclipseSwtPrinting"/>
		<rdfs:seeAlso rdf:resource="&swt-3_3;OrgEclipseSwtDnd"/>
		<rdfs:seeAlso rdf:resource="&swt-3_3;OrgEclipseSwtGraphics"/>
		<rdfs:comment xml:lang="en">Java API part implementing the org.eclipse.swt.custom package for SWT 3.3</rdfs:comment>
	</owl:Class>
	<owl:Class rdf:about="&swt-3_3;OrgEclipseSwtPrinting">
		<rdfs:subClassOf rdf:resource="&swt-3_2;OrgEclipseSwtPrinting"/>
		<rdfs:seeAlso rdf:resource="&swt-3_3;OrgEclipseSwtWidgets"/>
		<rdfs:seeAlso rdf:resource="&swt-3_3;OrgEclipseSwtGraphics"/>
		<rdfs:comment xml:lang="en">Java API part implementing the org.eclipse.swt.printing package for SWT 3.3</rdfs:comment>
	</owl:Class>
	<owl:Class rdf:about="&swt-3_3;OrgEclipseSwtDnd">
		<rdfs:subClassOf rdf:resource="&swt-3_2;OrgEclipseSwtDnd"/>
		<rdfs:seeAlso rdf:resource="&swt-3_3;OrgEclipseSwtEvents"/>
		<rdfs:seeAlso rdf:resource="&swt-3_3;OrgEclipseSwtWidgets"/>
		<rdfs:seeAlso rdf:resource="&swt-3_3;OrgEclipseSwtGraphics"/>
		<rdfs:comment xml:lang="en">Java API part implementing the org.eclipse.swt.dnd package for SWT 3.3</rdfs:comment>
	</owl:Class>
	<owl:Class rdf:about="&swt-3_3;OrgEclipseSwtLayout">
		<owl:equivalentClass rdf:resource="&swt-3_2;OrgEclipseSwtLayout"/>
		<rdfs:subClassOf rdf:resource="&java;JavaAPIPart"/>
		<rdfs:seeAlso rdf:resource="&swt-3_3;OrgEclipseSwtWidgets"/>
		<rdfs:seeAlso rdf:resource="&swt-3_3;OrgEclipseSwtGraphics"/>
		<rdfs:comment xml:lang="en">Java API part implementing the org.eclipse.swt.layout package for SWT 3.3</rdfs:comment>
	</owl:Class>
	<owl:Class rdf:about="&swt-3_3;OrgEclipseSwtOpengl">
		<rdfs:subClassOf rdf:resource="&swt-3_2;OrgEclipseSwtOpengl"/>
		<rdfs:seeAlso rdf:resource="&swt-3_3;OrgEclipseSwtWidgets"/>
		<rdfs:comment xml:lang="en">Java API part implementing the org.eclipse.swt.opengl package for SWT 3.3</rdfs:comment>
	</owl:Class>
	<owl:Class rdf:about="&swt-3_3;OrgEclipseSwtProgram">
		<owl:equivalentClass rdf:resource="&swt-3_2;OrgEclipseSwtProgram"/>
		<rdfs:subClassOf rdf:resource="&java;JavaAPIPart"/>
		<rdfs:seeAlso rdf:resource="&swt-3_3;OrgEclipseSwtGraphics"/>
		<rdfs:comment xml:lang="en">Java API part implementing the org.eclipse.swt.program package for SWT 3.3</rdfs:comment>
	</owl:Class>
	<owl:Class rdf:about="&swt-3_3;OrgEclipseSwtAPI">
		<rdfs:subClassOf rdf:resource="&swt-3_2;OrgEclipseSwtAPI"/>
		<rdfs:comment xml:lang="en">JavaLibrary implementing the org.eclipse.swt package for SWT 3.3</rdfs:comment>
		<rdfs:comment xml:lang="OWLManchester">platform:comprisesInterfacePart some OrgEclipseSwt</rdfs:comment>
	</owl:Class>
	<owl:Class rdf:about="&swt-3_3;OrgEclipseSwtAccessibilityAPI">
		<owl:equivalentClass rdf:resource="&swt-3_2;OrgEclipseSwtAccessibilityAPI"/>
		<rdfs:subClassOf rdf:resource="&java;JavaAPI"/>
		<rdfs:comment xml:lang="en">JavaLibrary implementing the org.eclipse.swt.accessibility package for SWT 3.3</rdfs:comment>
		<rdfs:comment xml:lang="OWLManchester">platform:comprisesInterfacePart some OrgEclipseSwtAccessibility</rdfs:comment>
	</owl:Class>
	<owl:Class rdf:about="&swt-3_3;OrgEclipseSwtWidgetsAPI">
		<rdfs:subClassOf rdf:resource="&swt-3_2;OrgEclipseSwtWidgetsAPI"/>
		<rdfs:comment xml:lang="en">JavaLibrary implementing the org.eclipse.swt.widgets package for SWT 3.3</rdfs:comment>
		<rdfs:comment xml:lang="OWLManchester">platform:comprisesInterfacePart some OrgEclipseSwtWidgets</rdfs:comment>
	</owl:Class>
	<owl:Class rdf:about="&swt-3_3;OrgEclipseSwtAwtAPI">
		<owl:equivalentClass rdf:resource="&swt-3_2;OrgEclipseSwtAwtAPI"/>
		<rdfs:subClassOf rdf:resource="&java;JavaAPI"/>
		<rdfs:comment xml:lang="en">JavaLibrary implementing the org.eclipse.swt.awt package for SWT 3.3</rdfs:comment>
		<rdfs:comment xml:lang="OWLManchester">platform:comprisesInterfacePart some OrgEclipseSwtAwt</rdfs:comment>
	</owl:Class>
	<owl:Class rdf:about="&swt-3_3;OrgEclipseSwtBrowserAPI">
		<rdfs:subClassOf rdf:resource="&swt-3_2;OrgEclipseSwtBrowserAPI"/>
		<rdfs:comment xml:lang="en">JavaLibrary implementing the org.eclipse.swt.browser package for SWT 3.3</rdfs:comment>
		<rdfs:comment xml:lang="OWLManchester">platform:comprisesInterfacePart some OrgEclipseSwtBrowser</rdfs:comment>
	</owl:Class>
	<owl:Class rdf:about="&swt-3_3;OrgEclipseSwtEventsAPI">
		<rdfs:subClassOf rdf:resource="&swt-3_2;OrgEclipseSwtEventsAPI"/>
		<rdfs:comment xml:lang="en">JavaLibrary implementing the org.eclipse.swt.events package for SWT 3.3</rdfs:comment>
		<rdfs:comment xml:lang="OWLManchester">platform:comprisesInterfacePart some OrgEclipseSwtEvents</rdfs:comment>
	</owl:Class>
	<owl:Class rdf:about="&swt-3_3;OrgEclipseSwtGraphicsAPI">
		<rdfs:subClassOf rdf:resource="&swt-3_2;OrgEclipseSwtGraphicsAPI"/>
		<rdfs:comment xml:lang="en">JavaLibrary implementing the org.eclipse.swt.graphics package for SWT 3.3</rdfs:comment>
		<rdfs:comment xml:lang="OWLManchester">platform:comprisesInterfacePart some OrgEclipseSwtGraphics</rdfs:comment>
	</owl:Class>
	<owl:Class rdf:about="&swt-3_3;OrgEclipseSwtCustomAPI">
		<rdfs:subClassOf rdf:resource="&swt-3_2;OrgEclipseSwtCustomAPI"/>
		<rdfs:comment xml:lang="en">JavaLibrary implementing the org.eclipse.swt.custom package for SWT 3.3</rdfs:comment>
		<rdfs:comment xml:lang="OWLManchester">platform:comprisesInterfacePart some OrgEclipseSwtCustom</rdfs:comment>
	</owl:Class>
	<owl:Class rdf:about="&swt-3_3;OrgEclipseSwtPrintingAPI">
		<rdfs:subClassOf rdf:resource="&swt-3_2;OrgEclipseSwtPrintingAPI"/>
		<rdfs:comment xml:lang="en">JavaLibrary implementing the org.eclipse.swt.printing package for SWT 3.3</rdfs:comment>
		<rdfs:comment xml:lang="OWLManchester">platform:comprisesInterfacePart some OrgEclipseSwtPrinting</rdfs:comment>
	</owl:Class>
	<owl:Class rdf:about="&swt-3_3;OrgEclipseSwtDndAPI">
		<rdfs:subClassOf rdf:resource="&swt-3_2;OrgEclipseSwtDndAPI"/>
		<rdfs:comment xml:lang="en">JavaLibrary implementing the org.eclipse.swt.dnd package for SWT 3.3</rdfs:comment>
		<rdfs:comment xml:lang="OWLManchester">platform:comprisesInterfacePart some OrgEclipseSwtDnd</rdfs:comment>
	</owl:Class>
	<owl:Class rdf:about="&swt-3_3;OrgEclipseSwtLayoutAPI">
		<owl:equivalentClass rdf:resource="&swt-3_2;OrgEclipseSwtLayoutAPI"/>
		<rdfs:subClassOf rdf:resource="&java;JavaAPI"/>
		<rdfs:comment xml:lang="en">JavaLibrary implementing the org.eclipse.swt.layout package for SWT 3.3</rdfs:comment>
		<rdfs:comment xml:lang="OWLManchester">platform:comprisesInterfacePart some OrgEclipseSwtLayout</rdfs:comment>
	</owl:Class>
	<owl:Class rdf:about="&swt-3_3;OrgEclipseSwtOpenglAPI">
		<rdfs:subClassOf rdf:resource="&swt-3_2;OrgEclipseSwtOpenglAPI"/>
		<rdfs:comment xml:lang="en">JavaLibrary implementing the org.eclipse.swt.opengl package for SWT 3.3</rdfs:comment>
		<rdfs:comment xml:lang="OWLManchester">platform:comprisesInterfacePart some OrgEclipseSwtOpengl</rdfs:comment>
	</owl:Class>
	<owl:Class rdf:about="&swt-3_3;OrgEclipseSwtProgramAPI">
		<owl:equivalentClass rdf:resource="&swt-3_2;OrgEclipseSwtProgramAPI"/>
		<rdfs:subClassOf rdf:resource="&java;JavaAPI"/>
		<rdfs:comment xml:lang="en">JavaLibrary implementing the org.eclipse.swt.program package for SWT 3.3</rdfs:comment>
		<rdfs:comment xml:lang="OWLManchester">platform:comprisesInterfacePart some OrgEclipseSwtProgram</rdfs:comment>
	</owl:Class>
	<swt-3_3:OrgEclipseSwt rdf:about="&swt-3_3;theOrgEclipseSwtPart">
	</swt-3_3:OrgEclipseSwt>
	<swt-3_3:OrgEclipseSwtAccessibility rdf:about="&swt-3_3;theOrgEclipseSwtAccessibilityPart">
	</swt-3_3:OrgEclipseSwtAccessibility>
	<swt-3_3:OrgEclipseSwtWidgets rdf:about="&swt-3_3;theOrgEclipseSwtWidgetsPart">
	</swt-3_3:OrgEclipseSwtWidgets>
	<swt-3_3:OrgEclipseSwtAwt rdf:about="&swt-3_3;theOrgEclipseSwtAwtPart">
	</swt-3_3:OrgEclipseSwtAwt>
	<swt-3_3:OrgEclipseSwtBrowser rdf:about="&swt-3_3;theOrgEclipseSwtBrowserPart">
	</swt-3_3:OrgEclipseSwtBrowser>
	<swt-3_3:OrgEclipseSwtEvents rdf:about="&swt-3_3;theOrgEclipseSwtEventsPart">
	</swt-3_3:OrgEclipseSwtEvents>
	<swt-3_3:OrgEclipseSwtGraphics rdf:about="&swt-3_3;theOrgEclipseSwtGraphicsPart">
	</swt-3_3:OrgEclipseSwtGraphics>
	<swt-3_3:OrgEclipseSwtCustom rdf:about="&swt-3_3;theOrgEclipseSwtCustomPart">
	</swt-3_3:OrgEclipseSwtCustom>
	<swt-3_3:OrgEclipseSwtPrinting rdf:about="&swt-3_3;theOrgEclipseSwtPrintingPart">
	</swt-3_3:OrgEclipseSwtPrinting>
	<swt-3_3:OrgEclipseSwtDnd rdf:about="&swt-3_3;theOrgEclipseSwtDndPart">
	</swt-3_3:OrgEclipseSwtDnd>
	<swt-3_3:OrgEclipseSwtLayout rdf:about="&swt-3_3;theOrgEclipseSwtLayoutPart">
	</swt-3_3:OrgEclipseSwtLayout>
	<swt-3_3:OrgEclipseSwtOpengl rdf:about="&swt-3_3;theOrgEclipseSwtOpenglPart">
	</swt-3_3:OrgEclipseSwtOpengl>
	<swt-3_3:OrgEclipseSwtProgram rdf:about="&swt-3_3;theOrgEclipseSwtProgramPart">
	</swt-3_3:OrgEclipseSwtProgram>
	<owl:Class rdf:about="&swt-3_3;OrgEclipseSwtClassLibrary">
		<rdfs:subClassOf rdf:resource="&swt-3_2;OrgEclipseSwtClassLibrary"/>
		<rdfs:comment xml:lang="en">JavaLibrary implementing the org.eclipse.swt package for SWT 3.3</rdfs:comment>
		<rdfs:comment xml:lang="OWLManchester">platform:implementsInterface some OrgEclipseSwtAPI</rdfs:comment>
	</owl:Class>
	<owl:Class rdf:about="&swt-3_3;OrgEclipseSwtAccessibilityClassLibrary">
		<owl:equivalentClass rdf:resource="&swt-3_2;OrgEclipseSwtAccessibilityClassLibrary"/>
		<rdfs:subClassOf rdf:resource="&java;JavaClassLibrary"/>
		<rdfs:comment xml:lang="en">JavaLibrary implementing the org.eclipse.swt.accessibility package for SWT 3.3</rdfs:comment>
		<rdfs:comment xml:lang="OWLManchester">platform:implementsInterface some OrgEclipseSwtAccessibilityAPI</rdfs:comment>
	</owl:Class>
	<owl:Class rdf:about="&swt-3_3;OrgEclipseSwtWidgetsClassLibrary">
		<rdfs:subClassOf rdf:resource="&swt-3_2;OrgEclipseSwtWidgetsClassLibrary"/>
		<rdfs:comment xml:lang="en">JavaLibrary implementing the org.eclipse.swt.widgets package for SWT 3.3</rdfs:comment>
		<rdfs:comment xml:lang="OWLManchester">platform:implementsInterface some OrgEclipseSwtWidgetsAPI</rdfs:comment>
	</owl:Class>
	<owl:Class rdf:about="&swt-3_3;OrgEclipseSwtAwtClassLibrary">
		<owl:equivalentClass rdf:resource="&swt-3_2;OrgEclipseSwtAwtClassLibrary"/>
		<rdfs:subClassOf rdf:resource="&java;JavaClassLibrary"/>
		<rdfs:comment xml:lang="en">JavaLibrary implementing the org.eclipse.swt.awt package for SWT 3.3</rdfs:comment>
		<rdfs:comment xml:lang="OWLManchester">platform:implementsInterface some OrgEclipseSwtAwtAPI</rdfs:comment>
	</owl:Class>
	<owl:Class rdf:about="&swt-3_3;OrgEclipseSwtBrowserClassLibrary">
		<rdfs:subClassOf rdf:resource="&swt-3_2;OrgEclipseSwtBrowserClassLibrary"/>
		<rdfs:comment xml:lang="en">JavaLibrary implementing the org.eclipse.swt.browser package for SWT 3.3</rdfs:comment>
		<rdfs:comment xml:lang="OWLManchester">platform:implementsInterface some OrgEclipseSwtBrowserAPI</rdfs:comment>
	</owl:Class>
	<owl:Class rdf:about="&swt-3_3;OrgEclipseSwtEventsClassLibrary">
		<rdfs:subClassOf rdf:resource="&swt-3_2;OrgEclipseSwtEventsClassLibrary"/>
		<rdfs:comment xml:lang="en">JavaLibrary implementing the org.eclipse.swt.events package for SWT 3.3</rdfs:comment>
		<rdfs:comment xml:lang="OWLManchester">platform:implementsInterface some OrgEclipseSwtEventsAPI</rdfs:comment>
	</owl:Class>
	<owl:Class rdf:about="&swt-3_3;OrgEclipseSwtGraphicsClassLibrary">
		<rdfs:subClassOf rdf:resource="&swt-3_2;OrgEclipseSwtGraphicsClassLibrary"/>
		<rdfs:comment xml:lang="en">JavaLibrary implementing the org.eclipse.swt.graphics package for SWT 3.3</rdfs:comment>
		<rdfs:comment xml:lang="OWLManchester">platform:implementsInterface some OrgEclipseSwtGraphicsAPI</rdfs:comment>
	</owl:Class>
	<owl:Class rdf:about="&swt-3_3;OrgEclipseSwtCustomClassLibrary">
		<rdfs:subClassOf rdf:resource="&swt-3_2;OrgEclipseSwtCustomClassLibrary"/>
		<rdfs:comment xml:lang="en">JavaLibrary implementing the org.eclipse.swt.custom package for SWT 3.3</rdfs:comment>
		<rdfs:comment xml:lang="OWLManchester">platform:implementsInterface some OrgEclipseSwtCustomAPI</rdfs:comment>
	</owl:Class>
	<owl:Class rdf:about="&swt-3_3;OrgEclipseSwtPrintingClassLibrary">
		<rdfs:subClassOf rdf:resource="&swt-3_2;OrgEclipseSwtPrintingClassLibrary"/>
		<rdfs:comment xml:lang="en">JavaLibrary implementing the org.eclipse.swt.printing package for SWT 3.3</rdfs:comment>
		<rdfs:comment xml:lang="OWLManchester">platform:implementsInterface some OrgEclipseSwtPrintingAPI</rdfs:comment>
	</owl:Class>
	<owl:Class rdf:about="&swt-3_3;OrgEclipseSwtDndClassLibrary">
		<rdfs:subClassOf rdf:resource="&swt-3_2;OrgEclipseSwtDndClassLibrary"/>
		<rdfs:comment xml:lang="en">JavaLibrary implementing the org.eclipse.swt.dnd package for SWT 3.3</rdfs:comment>
		<rdfs:comment xml:lang="OWLManchester">platform:implementsInterface some OrgEclipseSwtDndAPI</rdfs:comment>
	</owl:Class>
	<owl:Class rdf:about="&swt-3_3;OrgEclipseSwtLayoutClassLibrary">
		<owl:equivalentClass rdf:resource="&swt-3_2;OrgEclipseSwtLayoutClassLibrary"/>
		<rdfs:subClassOf rdf:resource="&java;JavaClassLibrary"/>
		<rdfs:comment xml:lang="en">JavaLibrary implementing the org.eclipse.swt.layout package for SWT 3.3</rdfs:comment>
		<rdfs:comment xml:lang="OWLManchester">platform:implementsInterface some OrgEclipseSwtLayoutAPI</rdfs:comment>
	</owl:Class>
	<owl:Class rdf:about="&swt-3_3;OrgEclipseSwtOpenglClassLibrary">
		<rdfs:subClassOf rdf:resource="&swt-3_2;OrgEclipseSwtOpenglClassLibrary"/>
		<rdfs:comment xml:lang="en">JavaLibrary implementing the org.eclipse.swt.opengl package for SWT 3.3</rdfs:comment>
		<rdfs:comment xml:lang="OWLManchester">platform:implementsInterface some OrgEclipseSwtOpenglAPI</rdfs:comment>
	</owl:Class>
	<owl:Class rdf:about="&swt-3_3;OrgEclipseSwtProgramClassLibrary">
		<owl:equivalentClass rdf:resource="&swt-3_2;OrgEclipseSwtProgramClassLibrary"/>
		<rdfs:subClassOf rdf:resource="&java;JavaClassLibrary"/>
		<rdfs:comment xml:lang="en">JavaLibrary implementing the org.eclipse.swt.program package for SWT 3.3</rdfs:comment>
		<rdfs:comment xml:lang="OWLManchester">platform:implementsInterface some OrgEclipseSwtProgramAPI</rdfs:comment>
	</owl:Class>
</rdf:RDF>
