<?xml version="1.0" encoding="ISO-8859-1"?>
<!DOCTYPE rdf:RDF [
	<!ENTITY java-se-6 "http://soft.vub.ac.be/platformkit/2010/1/java-se-6.owl#">
	<!ENTITY isa "http://localhost/~dennis/platformkit/2010_1/isa.owl#">
	<!ENTITY android-2_3 "http://soft.vub.ac.be/platformkit/2010/1/android-2_3.owl#">
	<!ENTITY ns_33 "http://localhost/~dennis/platformkit/2010_1/">
	<!ENTITY xsd "http://www.w3.org/2001/XMLSchema#">
	<!ENTITY platform "http://localhost/~dennis/platformkit/2010_1/platform.owl#">
	<!ENTITY android-2_2 "http://soft.vub.ac.be/platformkit/2010/1/android-2_2.owl#">
	<!ENTITY java "http://localhost/~dennis/platformkit/2010_1/java.owl#">
	<!ENTITY rdf "http://www.w3.org/1999/02/22-rdf-syntax-ns#">
	<!ENTITY rdfs "http://www.w3.org/2000/01/rdf-schema#">
	<!ENTITY owl "http://www.w3.org/2002/07/owl#">
]>
<rdf:RDF
	 xmlns:java-se-6="&java-se-6;"
	 xmlns:isa="&isa;"
	 xmlns:android-2_3="&android-2_3;"
	 xmlns:ns_33="&ns_33;"
	 xmlns:xsd="&xsd;"
	 xmlns:platform="&platform;"
	 xmlns:android-2_2="&android-2_2;"
	 xmlns:java="&java;"
	 xmlns:rdf="&rdf;"
	 xmlns:rdfs="&rdfs;"
	 xmlns:owl="&owl;"
>

	<owl:Ontology rdf:about="http://soft.vub.ac.be/platformkit/2010/1/android-2_3.owl#">
		<owl:versionInfo>$Id: UML2ToPackageAPIOntology.atl 8082 2010-03-18 21:11:00Z dwagelaa $</owl:versionInfo>
		<owl:imports rdf:resource="http://localhost/~dennis/platformkit/2010_1/platform.owl"/>
		<owl:imports rdf:resource="http://localhost/~dennis/platformkit/2010_1/java.owl"/>
		<owl:imports rdf:resource="http://soft.vub.ac.be/platformkit/2010/1/android-2_2.owl#"/>
		<owl:imports rdf:resource="http://localhost/~dennis/platformkit/2010_1/isa.owl"/>
		<owl:imports rdf:resource="http://soft.vub.ac.be/platformkit/2010/1/java-se-6.owl#"/>
		<rdfs:comment xml:lang="en">Generated by [UML2ToSimplifiedPackageAPIOntology.atl 8080 2010-03-18 10:46:40Z dwagelaa], [UML2ToPackageAPIOntology.atl 8082 2010-03-18 21:11:00Z dwagelaa], [UML2ToAPIOntology.atl 8086 2010-03-19 09:49:17Z dwagelaa], and [UML2Comparison.atl 8326 2010-11-11 13:32:14Z dwagelaa]</rdfs:comment>
		<rdfs:comment>Dennis Wagelaar &lt;dennis.wagelaar@vub.ac.be&gt;</rdfs:comment>
		<rdfs:comment xml:lang="en">&#169; 2010, Vrije Universiteit Brussel. All rights reserved.</rdfs:comment>
		<rdfs:label xml:lang="en">Android 2.3</rdfs:label>
	</owl:Ontology>
	<owl:Class rdf:about="&android-2_3;Android2_3API">
		<rdfs:subClassOf rdf:resource="&android-2_3;JavaxXmlAPI"/>
		<rdfs:subClassOf rdf:resource="&android-2_3;JavaxXmlDatatypeAPI"/>
		<rdfs:subClassOf rdf:resource="&android-2_3;JavaxXmlNamespaceAPI"/>
		<rdfs:subClassOf rdf:resource="&android-2_3;JavaxXmlXpathAPI"/>
		<rdfs:subClassOf rdf:resource="&android-2_3;JavaxXmlTransformAPI"/>
		<rdfs:subClassOf rdf:resource="&android-2_3;JavaxXmlTransformDomAPI"/>
		<rdfs:subClassOf rdf:resource="&android-2_3;JavaxXmlTransformSaxAPI"/>
		<rdfs:subClassOf rdf:resource="&android-2_3;JavaxXmlTransformStreamAPI"/>
		<rdfs:subClassOf rdf:resource="&android-2_3;JavaxXmlParsersAPI"/>
		<rdfs:subClassOf rdf:resource="&android-2_3;JavaxXmlValidationAPI"/>
		<rdfs:subClassOf rdf:resource="&android-2_3;JavaxSecurityCertAPI"/>
		<rdfs:subClassOf rdf:resource="&android-2_3;JavaxSecurityAuthAPI"/>
		<rdfs:subClassOf rdf:resource="&android-2_3;JavaxSecurityAuthCallbackAPI"/>
		<rdfs:subClassOf rdf:resource="&android-2_3;JavaxSecurityAuthLoginAPI"/>
		<rdfs:subClassOf rdf:resource="&android-2_3;JavaxSecurityAuthX500API"/>
		<rdfs:subClassOf rdf:resource="&android-2_3;JavaxSqlAPI"/>
		<rdfs:subClassOf rdf:resource="&android-2_3;JavaxCryptoAPI"/>
		<rdfs:subClassOf rdf:resource="&android-2_3;JavaxCryptoInterfacesAPI"/>
		<rdfs:subClassOf rdf:resource="&android-2_3;JavaxCryptoSpecAPI"/>
		<rdfs:subClassOf rdf:resource="&android-2_3;JavaxMicroeditionKhronosEglAPI"/>
		<rdfs:subClassOf rdf:resource="&android-2_3;JavaxMicroeditionKhronosOpenglesAPI"/>
		<rdfs:subClassOf rdf:resource="&android-2_3;JavaxNetAPI"/>
		<rdfs:subClassOf rdf:resource="&android-2_3;JavaxNetSslAPI"/>
		<rdfs:subClassOf rdf:resource="&android-2_3;JavaLangAPI"/>
		<rdfs:subClassOf rdf:resource="&android-2_3;JavaLangReflectAPI"/>
		<rdfs:subClassOf rdf:resource="&android-2_3;JavaLangAnnotationAPI"/>
		<rdfs:subClassOf rdf:resource="&android-2_3;JavaLangRefAPI"/>
		<rdfs:subClassOf rdf:resource="&android-2_3;JavaUtilAPI"/>
		<rdfs:subClassOf rdf:resource="&android-2_3;JavaUtilJarAPI"/>
		<rdfs:subClassOf rdf:resource="&android-2_3;JavaUtilZipAPI"/>
		<rdfs:subClassOf rdf:resource="&android-2_3;JavaUtilPrefsAPI"/>
		<rdfs:subClassOf rdf:resource="&android-2_3;JavaUtilRegexAPI"/>
		<rdfs:subClassOf rdf:resource="&android-2_3;JavaUtilConcurrentAPI"/>
		<rdfs:subClassOf rdf:resource="&android-2_3;JavaUtilConcurrentAtomicAPI"/>
		<rdfs:subClassOf rdf:resource="&android-2_3;JavaUtilConcurrentLocksAPI"/>
		<rdfs:subClassOf rdf:resource="&android-2_3;JavaUtilLoggingAPI"/>
		<rdfs:subClassOf rdf:resource="&android-2_3;JavaMathAPI"/>
		<rdfs:subClassOf rdf:resource="&android-2_3;JavaIoAPI"/>
		<rdfs:subClassOf rdf:resource="&android-2_3;JavaNetAPI"/>
		<rdfs:subClassOf rdf:resource="&android-2_3;JavaSecurityAPI"/>
		<rdfs:subClassOf rdf:resource="&android-2_3;JavaSecuritySpecAPI"/>
		<rdfs:subClassOf rdf:resource="&android-2_3;JavaSecurityCertAPI"/>
		<rdfs:subClassOf rdf:resource="&android-2_3;JavaSecurityInterfacesAPI"/>
		<rdfs:subClassOf rdf:resource="&android-2_3;JavaSecurityAclAPI"/>
		<rdfs:subClassOf rdf:resource="&android-2_3;JavaSqlAPI"/>
		<rdfs:subClassOf rdf:resource="&android-2_3;JavaNioAPI"/>
		<rdfs:subClassOf rdf:resource="&android-2_3;JavaNioChannelsAPI"/>
		<rdfs:subClassOf rdf:resource="&android-2_3;JavaNioChannelsSpiAPI"/>
		<rdfs:subClassOf rdf:resource="&android-2_3;JavaNioCharsetAPI"/>
		<rdfs:subClassOf rdf:resource="&android-2_3;JavaNioCharsetSpiAPI"/>
		<rdfs:subClassOf rdf:resource="&android-2_3;JavaBeansAPI"/>
		<rdfs:subClassOf rdf:resource="&android-2_3;JavaTextAPI"/>
		<rdfs:subClassOf rdf:resource="&android-2_3;JavaAwtFontAPI"/>
		<rdfs:subClassOf rdf:resource="&android-2_3;OrgXmlSaxAPI"/>
		<rdfs:subClassOf rdf:resource="&android-2_3;OrgXmlSaxExtAPI"/>
		<rdfs:subClassOf rdf:resource="&android-2_3;OrgXmlSaxHelpersAPI"/>
		<rdfs:subClassOf rdf:resource="&android-2_3;OrgW3cDomAPI"/>
		<rdfs:subClassOf rdf:resource="&android-2_3;OrgW3cDomLsAPI"/>
		<rdfs:subClassOf rdf:resource="&android-2_3;OrgXmlpullV1API"/>
		<rdfs:subClassOf rdf:resource="&android-2_3;OrgXmlpullV1Sax2API"/>
		<rdfs:subClassOf rdf:resource="&android-2_3;OrgApacheHttpAPI"/>
		<rdfs:subClassOf rdf:resource="&android-2_3;OrgApacheHttpClientAPI"/>
		<rdfs:subClassOf rdf:resource="&android-2_3;OrgApacheHttpClientMethodsAPI"/>
		<rdfs:subClassOf rdf:resource="&android-2_3;OrgApacheHttpClientEntityAPI"/>
		<rdfs:subClassOf rdf:resource="&android-2_3;OrgApacheHttpClientParamsAPI"/>
		<rdfs:subClassOf rdf:resource="&android-2_3;OrgApacheHttpClientProtocolAPI"/>
		<rdfs:subClassOf rdf:resource="&android-2_3;OrgApacheHttpClientUtilsAPI"/>
		<rdfs:subClassOf rdf:resource="&android-2_3;OrgApacheHttpParamsAPI"/>
		<rdfs:subClassOf rdf:resource="&android-2_3;OrgApacheHttpConnAPI"/>
		<rdfs:subClassOf rdf:resource="&android-2_3;OrgApacheHttpConnSslAPI"/>
		<rdfs:subClassOf rdf:resource="&android-2_3;OrgApacheHttpConnRoutingAPI"/>
		<rdfs:subClassOf rdf:resource="&android-2_3;OrgApacheHttpConnSchemeAPI"/>
		<rdfs:subClassOf rdf:resource="&android-2_3;OrgApacheHttpConnUtilAPI"/>
		<rdfs:subClassOf rdf:resource="&android-2_3;OrgApacheHttpConnParamsAPI"/>
		<rdfs:subClassOf rdf:resource="&android-2_3;OrgApacheHttpProtocolAPI"/>
		<rdfs:subClassOf rdf:resource="&android-2_3;OrgApacheHttpEntityAPI"/>
		<rdfs:subClassOf rdf:resource="&android-2_3;OrgApacheHttpImplAPI"/>
		<rdfs:subClassOf rdf:resource="&android-2_3;OrgApacheHttpImplEntityAPI"/>
		<rdfs:subClassOf rdf:resource="&android-2_3;OrgApacheHttpImplConnAPI"/>
		<rdfs:subClassOf rdf:resource="&android-2_3;OrgApacheHttpImplConnTsccmAPI"/>
		<rdfs:subClassOf rdf:resource="&android-2_3;OrgApacheHttpImplIoAPI"/>
		<rdfs:subClassOf rdf:resource="&android-2_3;OrgApacheHttpImplCookieAPI"/>
		<rdfs:subClassOf rdf:resource="&android-2_3;OrgApacheHttpImplAuthAPI"/>
		<rdfs:subClassOf rdf:resource="&android-2_3;OrgApacheHttpImplClientAPI"/>
		<rdfs:subClassOf rdf:resource="&android-2_3;OrgApacheHttpIoAPI"/>
		<rdfs:subClassOf rdf:resource="&android-2_3;OrgApacheHttpUtilAPI"/>
		<rdfs:subClassOf rdf:resource="&android-2_3;OrgApacheHttpMessageAPI"/>
		<rdfs:subClassOf rdf:resource="&android-2_3;OrgApacheHttpCookieAPI"/>
		<rdfs:subClassOf rdf:resource="&android-2_3;OrgApacheHttpCookieParamsAPI"/>
		<rdfs:subClassOf rdf:resource="&android-2_3;OrgApacheHttpAuthAPI"/>
		<rdfs:subClassOf rdf:resource="&android-2_3;OrgApacheHttpAuthParamsAPI"/>
		<rdfs:subClassOf rdf:resource="&android-2_3;OrgApacheCommonsLoggingAPI"/>
		<rdfs:subClassOf rdf:resource="&android-2_3;OrgJsonAPI"/>
		<rdfs:subClassOf rdf:resource="&android-2_3;DalvikBytecodeAPI"/>
		<rdfs:subClassOf rdf:resource="&android-2_3;DalvikAnnotationAPI"/>
		<rdfs:subClassOf rdf:resource="&android-2_3;DalvikSystemAPI"/>
		<rdfs:subClassOf rdf:resource="&android-2_3;JunitRunnerAPI"/>
		<rdfs:subClassOf rdf:resource="&android-2_3;JunitFrameworkAPI"/>
		<rdfs:subClassOf rdf:resource="&android-2_3;AndroidAPI"/>
		<rdfs:subClassOf rdf:resource="&android-2_3;AndroidContentAPI"/>
		<rdfs:subClassOf rdf:resource="&android-2_3;AndroidContentPmAPI"/>
		<rdfs:subClassOf rdf:resource="&android-2_3;AndroidContentResAPI"/>
		<rdfs:subClassOf rdf:resource="&android-2_3;AndroidOsAPI"/>
		<rdfs:subClassOf rdf:resource="&android-2_3;AndroidOsStorageAPI"/>
		<rdfs:subClassOf rdf:resource="&android-2_3;AndroidAccountsAPI"/>
		<rdfs:subClassOf rdf:resource="&android-2_3;AndroidNetAPI"/>
		<rdfs:subClassOf rdf:resource="&android-2_3;AndroidNetHttpAPI"/>
		<rdfs:subClassOf rdf:resource="&android-2_3;AndroidNetSipAPI"/>
		<rdfs:subClassOf rdf:resource="&android-2_3;AndroidNetWifiAPI"/>
		<rdfs:subClassOf rdf:resource="&android-2_3;AndroidDatabaseAPI"/>
		<rdfs:subClassOf rdf:resource="&android-2_3;AndroidDatabaseSqliteAPI"/>
		<rdfs:subClassOf rdf:resource="&android-2_3;AndroidUtilAPI"/>
		<rdfs:subClassOf rdf:resource="&android-2_3;AndroidGraphicsAPI"/>
		<rdfs:subClassOf rdf:resource="&android-2_3;AndroidGraphicsDrawableAPI"/>
		<rdfs:subClassOf rdf:resource="&android-2_3;AndroidGraphicsDrawableShapesAPI"/>
		<rdfs:subClassOf rdf:resource="&android-2_3;AndroidViewAPI"/>
		<rdfs:subClassOf rdf:resource="&android-2_3;AndroidViewAccessibilityAPI"/>
		<rdfs:subClassOf rdf:resource="&android-2_3;AndroidViewInputmethodAPI"/>
		<rdfs:subClassOf rdf:resource="&android-2_3;AndroidViewAnimationAPI"/>
		<rdfs:subClassOf rdf:resource="&android-2_3;AndroidAccessibilityserviceAPI"/>
		<rdfs:subClassOf rdf:resource="&android-2_3;AndroidAppAPI"/>
		<rdfs:subClassOf rdf:resource="&android-2_3;AndroidAppBackupAPI"/>
		<rdfs:subClassOf rdf:resource="&android-2_3;AndroidAppAdminAPI"/>
		<rdfs:subClassOf rdf:resource="&android-2_3;AndroidTelephonyAPI"/>
		<rdfs:subClassOf rdf:resource="&android-2_3;AndroidTelephonyCdmaAPI"/>
		<rdfs:subClassOf rdf:resource="&android-2_3;AndroidTelephonyGsmAPI"/>
		<rdfs:subClassOf rdf:resource="&android-2_3;AndroidTextAPI"/>
		<rdfs:subClassOf rdf:resource="&android-2_3;AndroidTextUtilAPI"/>
		<rdfs:subClassOf rdf:resource="&android-2_3;AndroidTextFormatAPI"/>
		<rdfs:subClassOf rdf:resource="&android-2_3;AndroidTextMethodAPI"/>
		<rdfs:subClassOf rdf:resource="&android-2_3;AndroidTextStyleAPI"/>
		<rdfs:subClassOf rdf:resource="&android-2_3;AndroidGestureAPI"/>
		<rdfs:subClassOf rdf:resource="&android-2_3;AndroidWidgetAPI"/>
		<rdfs:subClassOf rdf:resource="&android-2_3;AndroidLocationAPI"/>
		<rdfs:subClassOf rdf:resource="&android-2_3;AndroidHardwareAPI"/>
		<rdfs:subClassOf rdf:resource="&android-2_3;AndroidWebkitAPI"/>
		<rdfs:subClassOf rdf:resource="&android-2_3;AndroidTestAPI"/>
		<rdfs:subClassOf rdf:resource="&android-2_3;AndroidTestMockAPI"/>
		<rdfs:subClassOf rdf:resource="&android-2_3;AndroidTestSuitebuilderAPI"/>
		<rdfs:subClassOf rdf:resource="&android-2_3;AndroidTestSuitebuilderAnnotationAPI"/>
		<rdfs:subClassOf rdf:resource="&android-2_3;AndroidPreferenceAPI"/>
		<rdfs:subClassOf rdf:resource="&android-2_3;AndroidMediaAPI"/>
		<rdfs:subClassOf rdf:resource="&android-2_3;AndroidMediaAudiofxAPI"/>
		<rdfs:subClassOf rdf:resource="&android-2_3;AndroidInputmethodserviceAPI"/>
		<rdfs:subClassOf rdf:resource="&android-2_3;AndroidServiceWallpaperAPI"/>
		<rdfs:subClassOf rdf:resource="&android-2_3;AndroidBluetoothAPI"/>
		<rdfs:subClassOf rdf:resource="&android-2_3;AndroidNfcAPI"/>
		<rdfs:subClassOf rdf:resource="&android-2_3;AndroidProviderAPI"/>
		<rdfs:subClassOf rdf:resource="&android-2_3;AndroidSaxAPI"/>
		<rdfs:subClassOf rdf:resource="&android-2_3;AndroidAppwidgetAPI"/>
		<rdfs:subClassOf rdf:resource="&android-2_3;AndroidOpenglAPI"/>
		<rdfs:subClassOf rdf:resource="&android-2_3;AndroidSpeechAPI"/>
		<rdfs:subClassOf rdf:resource="&android-2_3;AndroidSpeechTtsAPI"/>
		<rdfs:comment xml:lang="en">Android 2.3 API</rdfs:comment>
		<rdfs:comment xml:lang="OWLManchester">platform:comprisesInterfacePart some JavaxXml and platform:comprisesInterfacePart some JavaxXmlDatatype and platform:comprisesInterfacePart some JavaxXmlNamespace and platform:comprisesInterfacePart some JavaxXmlXpath and platform:comprisesInterfacePart some JavaxXmlTransform and platform:comprisesInterfacePart some JavaxXmlTransformDom and platform:comprisesInterfacePart some JavaxXmlTransformSax and platform:comprisesInterfacePart some JavaxXmlTransformStream and platform:comprisesInterfacePart some JavaxXmlParsers and platform:comprisesInterfacePart some JavaxXmlValidation and platform:comprisesInterfacePart some JavaxSecurityCert and platform:comprisesInterfacePart some JavaxSecurityAuth and platform:comprisesInterfacePart some JavaxSecurityAuthCallback and platform:comprisesInterfacePart some JavaxSecurityAuthLogin and platform:comprisesInterfacePart some JavaxSecurityAuthX500 and platform:comprisesInterfacePart some JavaxSql and platform:comprisesInterfacePart some JavaxCrypto and platform:comprisesInterfacePart some JavaxCryptoInterfaces and platform:comprisesInterfacePart some JavaxCryptoSpec and platform:comprisesInterfacePart some JavaxMicroeditionKhronosEgl and platform:comprisesInterfacePart some JavaxMicroeditionKhronosOpengles and platform:comprisesInterfacePart some JavaxNet and platform:comprisesInterfacePart some JavaxNetSsl and platform:comprisesInterfacePart some JavaLang and platform:comprisesInterfacePart some JavaLangReflect and platform:comprisesInterfacePart some JavaLangAnnotation and platform:comprisesInterfacePart some JavaLangRef and platform:comprisesInterfacePart some JavaUtil and platform:comprisesInterfacePart some JavaUtilJar and platform:comprisesInterfacePart some JavaUtilZip and platform:comprisesInterfacePart some JavaUtilPrefs and platform:comprisesInterfacePart some JavaUtilRegex and platform:comprisesInterfacePart some JavaUtilConcurrent and platform:comprisesInterfacePart some JavaUtilConcurrentAtomic and platform:comprisesInterfacePart some JavaUtilConcurrentLocks and platform:comprisesInterfacePart some JavaUtilLogging and platform:comprisesInterfacePart some JavaMath and platform:comprisesInterfacePart some JavaIo and platform:comprisesInterfacePart some JavaNet and platform:comprisesInterfacePart some JavaSecurity and platform:comprisesInterfacePart some JavaSecuritySpec and platform:comprisesInterfacePart some JavaSecurityCert and platform:comprisesInterfacePart some JavaSecurityInterfaces and platform:comprisesInterfacePart some JavaSecurityAcl and platform:comprisesInterfacePart some JavaSql and platform:comprisesInterfacePart some JavaNio and platform:comprisesInterfacePart some JavaNioChannels and platform:comprisesInterfacePart some JavaNioChannelsSpi and platform:comprisesInterfacePart some JavaNioCharset and platform:comprisesInterfacePart some JavaNioCharsetSpi and platform:comprisesInterfacePart some JavaBeans and platform:comprisesInterfacePart some JavaText and platform:comprisesInterfacePart some JavaAwtFont and platform:comprisesInterfacePart some OrgXmlSax and platform:comprisesInterfacePart some OrgXmlSaxExt and platform:comprisesInterfacePart some OrgXmlSaxHelpers and platform:comprisesInterfacePart some OrgW3cDom and platform:comprisesInterfacePart some OrgW3cDomLs and platform:comprisesInterfacePart some OrgXmlpullV1 and platform:comprisesInterfacePart some OrgXmlpullV1Sax2 and platform:comprisesInterfacePart some OrgApacheHttp and platform:comprisesInterfacePart some OrgApacheHttpClient and platform:comprisesInterfacePart some OrgApacheHttpClientMethods and platform:comprisesInterfacePart some OrgApacheHttpClientEntity and platform:comprisesInterfacePart some OrgApacheHttpClientParams and platform:comprisesInterfacePart some OrgApacheHttpClientProtocol and platform:comprisesInterfacePart some OrgApacheHttpClientUtils and platform:comprisesInterfacePart some OrgApacheHttpParams and platform:comprisesInterfacePart some OrgApacheHttpConn and platform:comprisesInterfacePart some OrgApacheHttpConnSsl and platform:comprisesInterfacePart some OrgApacheHttpConnRouting and platform:comprisesInterfacePart some OrgApacheHttpConnScheme and platform:comprisesInterfacePart some OrgApacheHttpConnUtil and platform:comprisesInterfacePart some OrgApacheHttpConnParams and platform:comprisesInterfacePart some OrgApacheHttpProtocol and platform:comprisesInterfacePart some OrgApacheHttpEntity and platform:comprisesInterfacePart some OrgApacheHttpImpl and platform:comprisesInterfacePart some OrgApacheHttpImplEntity and platform:comprisesInterfacePart some OrgApacheHttpImplConn and platform:comprisesInterfacePart some OrgApacheHttpImplConnTsccm and platform:comprisesInterfacePart some OrgApacheHttpImplIo and platform:comprisesInterfacePart some OrgApacheHttpImplCookie and platform:comprisesInterfacePart some OrgApacheHttpImplAuth and platform:comprisesInterfacePart some OrgApacheHttpImplClient and platform:comprisesInterfacePart some OrgApacheHttpIo and platform:comprisesInterfacePart some OrgApacheHttpUtil and platform:comprisesInterfacePart some OrgApacheHttpMessage and platform:comprisesInterfacePart some OrgApacheHttpCookie and platform:comprisesInterfacePart some OrgApacheHttpCookieParams and platform:comprisesInterfacePart some OrgApacheHttpAuth and platform:comprisesInterfacePart some OrgApacheHttpAuthParams and platform:comprisesInterfacePart some OrgApacheCommonsLogging and platform:comprisesInterfacePart some OrgJson and platform:comprisesInterfacePart some DalvikBytecode and platform:comprisesInterfacePart some DalvikAnnotation and platform:comprisesInterfacePart some DalvikSystem and platform:comprisesInterfacePart some JunitRunner and platform:comprisesInterfacePart some JunitFramework and platform:comprisesInterfacePart some Android and platform:comprisesInterfacePart some AndroidContent and platform:comprisesInterfacePart some AndroidContentPm and platform:comprisesInterfacePart some AndroidContentRes and platform:comprisesInterfacePart some AndroidOs and platform:comprisesInterfacePart some AndroidOsStorage and platform:comprisesInterfacePart some AndroidAccounts and platform:comprisesInterfacePart some AndroidNet and platform:comprisesInterfacePart some AndroidNetHttp and platform:comprisesInterfacePart some AndroidNetSip and platform:comprisesInterfacePart some AndroidNetWifi and platform:comprisesInterfacePart some AndroidDatabase and platform:comprisesInterfacePart some AndroidDatabaseSqlite and platform:comprisesInterfacePart some AndroidUtil and platform:comprisesInterfacePart some AndroidGraphics and platform:comprisesInterfacePart some AndroidGraphicsDrawable and platform:comprisesInterfacePart some AndroidGraphicsDrawableShapes and platform:comprisesInterfacePart some AndroidView and platform:comprisesInterfacePart some AndroidViewAccessibility and platform:comprisesInterfacePart some AndroidViewInputmethod and platform:comprisesInterfacePart some AndroidViewAnimation and platform:comprisesInterfacePart some AndroidAccessibilityservice and platform:comprisesInterfacePart some AndroidApp and platform:comprisesInterfacePart some AndroidAppBackup and platform:comprisesInterfacePart some AndroidAppAdmin and platform:comprisesInterfacePart some AndroidTelephony and platform:comprisesInterfacePart some AndroidTelephonyCdma and platform:comprisesInterfacePart some AndroidTelephonyGsm and platform:comprisesInterfacePart some AndroidText and platform:comprisesInterfacePart some AndroidTextUtil and platform:comprisesInterfacePart some AndroidTextFormat and platform:comprisesInterfacePart some AndroidTextMethod and platform:comprisesInterfacePart some AndroidTextStyle and platform:comprisesInterfacePart some AndroidGesture and platform:comprisesInterfacePart some AndroidWidget and platform:comprisesInterfacePart some AndroidLocation and platform:comprisesInterfacePart some AndroidHardware and platform:comprisesInterfacePart some AndroidWebkit and platform:comprisesInterfacePart some AndroidTest and platform:comprisesInterfacePart some AndroidTestMock and platform:comprisesInterfacePart some AndroidTestSuitebuilder and platform:comprisesInterfacePart some AndroidTestSuitebuilderAnnotation and platform:comprisesInterfacePart some AndroidPreference and platform:comprisesInterfacePart some AndroidMedia and platform:comprisesInterfacePart some AndroidMediaAudiofx and platform:comprisesInterfacePart some AndroidInputmethodservice and platform:comprisesInterfacePart some AndroidServiceWallpaper and platform:comprisesInterfacePart some AndroidBluetooth and platform:comprisesInterfacePart some AndroidNfc and platform:comprisesInterfacePart some AndroidProvider and platform:comprisesInterfacePart some AndroidSax and platform:comprisesInterfacePart some AndroidAppwidget and platform:comprisesInterfacePart some AndroidOpengl and platform:comprisesInterfacePart some AndroidSpeech and platform:comprisesInterfacePart some AndroidSpeechTts</rdfs:comment>
	</owl:Class>
	<owl:Class rdf:about="&android-2_3;Android2_3ClassLibrary">
		<rdfs:subClassOf rdf:resource="&android-2_3;JavaxXmlClassLibrary"/>
		<rdfs:subClassOf rdf:resource="&android-2_3;JavaxXmlDatatypeClassLibrary"/>
		<rdfs:subClassOf rdf:resource="&android-2_3;JavaxXmlNamespaceClassLibrary"/>
		<rdfs:subClassOf rdf:resource="&android-2_3;JavaxXmlXpathClassLibrary"/>
		<rdfs:subClassOf rdf:resource="&android-2_3;JavaxXmlTransformClassLibrary"/>
		<rdfs:subClassOf rdf:resource="&android-2_3;JavaxXmlTransformDomClassLibrary"/>
		<rdfs:subClassOf rdf:resource="&android-2_3;JavaxXmlTransformSaxClassLibrary"/>
		<rdfs:subClassOf rdf:resource="&android-2_3;JavaxXmlTransformStreamClassLibrary"/>
		<rdfs:subClassOf rdf:resource="&android-2_3;JavaxXmlParsersClassLibrary"/>
		<rdfs:subClassOf rdf:resource="&android-2_3;JavaxXmlValidationClassLibrary"/>
		<rdfs:subClassOf rdf:resource="&android-2_3;JavaxSecurityCertClassLibrary"/>
		<rdfs:subClassOf rdf:resource="&android-2_3;JavaxSecurityAuthClassLibrary"/>
		<rdfs:subClassOf rdf:resource="&android-2_3;JavaxSecurityAuthCallbackClassLibrary"/>
		<rdfs:subClassOf rdf:resource="&android-2_3;JavaxSecurityAuthLoginClassLibrary"/>
		<rdfs:subClassOf rdf:resource="&android-2_3;JavaxSecurityAuthX500ClassLibrary"/>
		<rdfs:subClassOf rdf:resource="&android-2_3;JavaxSqlClassLibrary"/>
		<rdfs:subClassOf rdf:resource="&android-2_3;JavaxCryptoClassLibrary"/>
		<rdfs:subClassOf rdf:resource="&android-2_3;JavaxCryptoInterfacesClassLibrary"/>
		<rdfs:subClassOf rdf:resource="&android-2_3;JavaxCryptoSpecClassLibrary"/>
		<rdfs:subClassOf rdf:resource="&android-2_3;JavaxMicroeditionKhronosEglClassLibrary"/>
		<rdfs:subClassOf rdf:resource="&android-2_3;JavaxMicroeditionKhronosOpenglesClassLibrary"/>
		<rdfs:subClassOf rdf:resource="&android-2_3;JavaxNetClassLibrary"/>
		<rdfs:subClassOf rdf:resource="&android-2_3;JavaxNetSslClassLibrary"/>
		<rdfs:subClassOf rdf:resource="&android-2_3;JavaLangClassLibrary"/>
		<rdfs:subClassOf rdf:resource="&android-2_3;JavaLangReflectClassLibrary"/>
		<rdfs:subClassOf rdf:resource="&android-2_3;JavaLangAnnotationClassLibrary"/>
		<rdfs:subClassOf rdf:resource="&android-2_3;JavaLangRefClassLibrary"/>
		<rdfs:subClassOf rdf:resource="&android-2_3;JavaUtilClassLibrary"/>
		<rdfs:subClassOf rdf:resource="&android-2_3;JavaUtilJarClassLibrary"/>
		<rdfs:subClassOf rdf:resource="&android-2_3;JavaUtilZipClassLibrary"/>
		<rdfs:subClassOf rdf:resource="&android-2_3;JavaUtilPrefsClassLibrary"/>
		<rdfs:subClassOf rdf:resource="&android-2_3;JavaUtilRegexClassLibrary"/>
		<rdfs:subClassOf rdf:resource="&android-2_3;JavaUtilConcurrentClassLibrary"/>
		<rdfs:subClassOf rdf:resource="&android-2_3;JavaUtilConcurrentAtomicClassLibrary"/>
		<rdfs:subClassOf rdf:resource="&android-2_3;JavaUtilConcurrentLocksClassLibrary"/>
		<rdfs:subClassOf rdf:resource="&android-2_3;JavaUtilLoggingClassLibrary"/>
		<rdfs:subClassOf rdf:resource="&android-2_3;JavaMathClassLibrary"/>
		<rdfs:subClassOf rdf:resource="&android-2_3;JavaIoClassLibrary"/>
		<rdfs:subClassOf rdf:resource="&android-2_3;JavaNetClassLibrary"/>
		<rdfs:subClassOf rdf:resource="&android-2_3;JavaSecurityClassLibrary"/>
		<rdfs:subClassOf rdf:resource="&android-2_3;JavaSecuritySpecClassLibrary"/>
		<rdfs:subClassOf rdf:resource="&android-2_3;JavaSecurityCertClassLibrary"/>
		<rdfs:subClassOf rdf:resource="&android-2_3;JavaSecurityInterfacesClassLibrary"/>
		<rdfs:subClassOf rdf:resource="&android-2_3;JavaSecurityAclClassLibrary"/>
		<rdfs:subClassOf rdf:resource="&android-2_3;JavaSqlClassLibrary"/>
		<rdfs:subClassOf rdf:resource="&android-2_3;JavaNioClassLibrary"/>
		<rdfs:subClassOf rdf:resource="&android-2_3;JavaNioChannelsClassLibrary"/>
		<rdfs:subClassOf rdf:resource="&android-2_3;JavaNioChannelsSpiClassLibrary"/>
		<rdfs:subClassOf rdf:resource="&android-2_3;JavaNioCharsetClassLibrary"/>
		<rdfs:subClassOf rdf:resource="&android-2_3;JavaNioCharsetSpiClassLibrary"/>
		<rdfs:subClassOf rdf:resource="&android-2_3;JavaBeansClassLibrary"/>
		<rdfs:subClassOf rdf:resource="&android-2_3;JavaTextClassLibrary"/>
		<rdfs:subClassOf rdf:resource="&android-2_3;JavaAwtFontClassLibrary"/>
		<rdfs:subClassOf rdf:resource="&android-2_3;OrgXmlSaxClassLibrary"/>
		<rdfs:subClassOf rdf:resource="&android-2_3;OrgXmlSaxExtClassLibrary"/>
		<rdfs:subClassOf rdf:resource="&android-2_3;OrgXmlSaxHelpersClassLibrary"/>
		<rdfs:subClassOf rdf:resource="&android-2_3;OrgW3cDomClassLibrary"/>
		<rdfs:subClassOf rdf:resource="&android-2_3;OrgW3cDomLsClassLibrary"/>
		<rdfs:subClassOf rdf:resource="&android-2_3;OrgXmlpullV1ClassLibrary"/>
		<rdfs:subClassOf rdf:resource="&android-2_3;OrgXmlpullV1Sax2ClassLibrary"/>
		<rdfs:subClassOf rdf:resource="&android-2_3;OrgApacheHttpClassLibrary"/>
		<rdfs:subClassOf rdf:resource="&android-2_3;OrgApacheHttpClientClassLibrary"/>
		<rdfs:subClassOf rdf:resource="&android-2_3;OrgApacheHttpClientMethodsClassLibrary"/>
		<rdfs:subClassOf rdf:resource="&android-2_3;OrgApacheHttpClientEntityClassLibrary"/>
		<rdfs:subClassOf rdf:resource="&android-2_3;OrgApacheHttpClientParamsClassLibrary"/>
		<rdfs:subClassOf rdf:resource="&android-2_3;OrgApacheHttpClientProtocolClassLibrary"/>
		<rdfs:subClassOf rdf:resource="&android-2_3;OrgApacheHttpClientUtilsClassLibrary"/>
		<rdfs:subClassOf rdf:resource="&android-2_3;OrgApacheHttpParamsClassLibrary"/>
		<rdfs:subClassOf rdf:resource="&android-2_3;OrgApacheHttpConnClassLibrary"/>
		<rdfs:subClassOf rdf:resource="&android-2_3;OrgApacheHttpConnSslClassLibrary"/>
		<rdfs:subClassOf rdf:resource="&android-2_3;OrgApacheHttpConnRoutingClassLibrary"/>
		<rdfs:subClassOf rdf:resource="&android-2_3;OrgApacheHttpConnSchemeClassLibrary"/>
		<rdfs:subClassOf rdf:resource="&android-2_3;OrgApacheHttpConnUtilClassLibrary"/>
		<rdfs:subClassOf rdf:resource="&android-2_3;OrgApacheHttpConnParamsClassLibrary"/>
		<rdfs:subClassOf rdf:resource="&android-2_3;OrgApacheHttpProtocolClassLibrary"/>
		<rdfs:subClassOf rdf:resource="&android-2_3;OrgApacheHttpEntityClassLibrary"/>
		<rdfs:subClassOf rdf:resource="&android-2_3;OrgApacheHttpImplClassLibrary"/>
		<rdfs:subClassOf rdf:resource="&android-2_3;OrgApacheHttpImplEntityClassLibrary"/>
		<rdfs:subClassOf rdf:resource="&android-2_3;OrgApacheHttpImplConnClassLibrary"/>
		<rdfs:subClassOf rdf:resource="&android-2_3;OrgApacheHttpImplConnTsccmClassLibrary"/>
		<rdfs:subClassOf rdf:resource="&android-2_3;OrgApacheHttpImplIoClassLibrary"/>
		<rdfs:subClassOf rdf:resource="&android-2_3;OrgApacheHttpImplCookieClassLibrary"/>
		<rdfs:subClassOf rdf:resource="&android-2_3;OrgApacheHttpImplAuthClassLibrary"/>
		<rdfs:subClassOf rdf:resource="&android-2_3;OrgApacheHttpImplClientClassLibrary"/>
		<rdfs:subClassOf rdf:resource="&android-2_3;OrgApacheHttpIoClassLibrary"/>
		<rdfs:subClassOf rdf:resource="&android-2_3;OrgApacheHttpUtilClassLibrary"/>
		<rdfs:subClassOf rdf:resource="&android-2_3;OrgApacheHttpMessageClassLibrary"/>
		<rdfs:subClassOf rdf:resource="&android-2_3;OrgApacheHttpCookieClassLibrary"/>
		<rdfs:subClassOf rdf:resource="&android-2_3;OrgApacheHttpCookieParamsClassLibrary"/>
		<rdfs:subClassOf rdf:resource="&android-2_3;OrgApacheHttpAuthClassLibrary"/>
		<rdfs:subClassOf rdf:resource="&android-2_3;OrgApacheHttpAuthParamsClassLibrary"/>
		<rdfs:subClassOf rdf:resource="&android-2_3;OrgApacheCommonsLoggingClassLibrary"/>
		<rdfs:subClassOf rdf:resource="&android-2_3;OrgJsonClassLibrary"/>
		<rdfs:subClassOf rdf:resource="&android-2_3;DalvikBytecodeClassLibrary"/>
		<rdfs:subClassOf rdf:resource="&android-2_3;DalvikAnnotationClassLibrary"/>
		<rdfs:subClassOf rdf:resource="&android-2_3;DalvikSystemClassLibrary"/>
		<rdfs:subClassOf rdf:resource="&android-2_3;JunitRunnerClassLibrary"/>
		<rdfs:subClassOf rdf:resource="&android-2_3;JunitFrameworkClassLibrary"/>
		<rdfs:subClassOf rdf:resource="&android-2_3;AndroidClassLibrary"/>
		<rdfs:subClassOf rdf:resource="&android-2_3;AndroidContentClassLibrary"/>
		<rdfs:subClassOf rdf:resource="&android-2_3;AndroidContentPmClassLibrary"/>
		<rdfs:subClassOf rdf:resource="&android-2_3;AndroidContentResClassLibrary"/>
		<rdfs:subClassOf rdf:resource="&android-2_3;AndroidOsClassLibrary"/>
		<rdfs:subClassOf rdf:resource="&android-2_3;AndroidOsStorageClassLibrary"/>
		<rdfs:subClassOf rdf:resource="&android-2_3;AndroidAccountsClassLibrary"/>
		<rdfs:subClassOf rdf:resource="&android-2_3;AndroidNetClassLibrary"/>
		<rdfs:subClassOf rdf:resource="&android-2_3;AndroidNetHttpClassLibrary"/>
		<rdfs:subClassOf rdf:resource="&android-2_3;AndroidNetSipClassLibrary"/>
		<rdfs:subClassOf rdf:resource="&android-2_3;AndroidNetWifiClassLibrary"/>
		<rdfs:subClassOf rdf:resource="&android-2_3;AndroidDatabaseClassLibrary"/>
		<rdfs:subClassOf rdf:resource="&android-2_3;AndroidDatabaseSqliteClassLibrary"/>
		<rdfs:subClassOf rdf:resource="&android-2_3;AndroidUtilClassLibrary"/>
		<rdfs:subClassOf rdf:resource="&android-2_3;AndroidGraphicsClassLibrary"/>
		<rdfs:subClassOf rdf:resource="&android-2_3;AndroidGraphicsDrawableClassLibrary"/>
		<rdfs:subClassOf rdf:resource="&android-2_3;AndroidGraphicsDrawableShapesClassLibrary"/>
		<rdfs:subClassOf rdf:resource="&android-2_3;AndroidViewClassLibrary"/>
		<rdfs:subClassOf rdf:resource="&android-2_3;AndroidViewAccessibilityClassLibrary"/>
		<rdfs:subClassOf rdf:resource="&android-2_3;AndroidViewInputmethodClassLibrary"/>
		<rdfs:subClassOf rdf:resource="&android-2_3;AndroidViewAnimationClassLibrary"/>
		<rdfs:subClassOf rdf:resource="&android-2_3;AndroidAccessibilityserviceClassLibrary"/>
		<rdfs:subClassOf rdf:resource="&android-2_3;AndroidAppClassLibrary"/>
		<rdfs:subClassOf rdf:resource="&android-2_3;AndroidAppBackupClassLibrary"/>
		<rdfs:subClassOf rdf:resource="&android-2_3;AndroidAppAdminClassLibrary"/>
		<rdfs:subClassOf rdf:resource="&android-2_3;AndroidTelephonyClassLibrary"/>
		<rdfs:subClassOf rdf:resource="&android-2_3;AndroidTelephonyCdmaClassLibrary"/>
		<rdfs:subClassOf rdf:resource="&android-2_3;AndroidTelephonyGsmClassLibrary"/>
		<rdfs:subClassOf rdf:resource="&android-2_3;AndroidTextClassLibrary"/>
		<rdfs:subClassOf rdf:resource="&android-2_3;AndroidTextUtilClassLibrary"/>
		<rdfs:subClassOf rdf:resource="&android-2_3;AndroidTextFormatClassLibrary"/>
		<rdfs:subClassOf rdf:resource="&android-2_3;AndroidTextMethodClassLibrary"/>
		<rdfs:subClassOf rdf:resource="&android-2_3;AndroidTextStyleClassLibrary"/>
		<rdfs:subClassOf rdf:resource="&android-2_3;AndroidGestureClassLibrary"/>
		<rdfs:subClassOf rdf:resource="&android-2_3;AndroidWidgetClassLibrary"/>
		<rdfs:subClassOf rdf:resource="&android-2_3;AndroidLocationClassLibrary"/>
		<rdfs:subClassOf rdf:resource="&android-2_3;AndroidHardwareClassLibrary"/>
		<rdfs:subClassOf rdf:resource="&android-2_3;AndroidWebkitClassLibrary"/>
		<rdfs:subClassOf rdf:resource="&android-2_3;AndroidTestClassLibrary"/>
		<rdfs:subClassOf rdf:resource="&android-2_3;AndroidTestMockClassLibrary"/>
		<rdfs:subClassOf rdf:resource="&android-2_3;AndroidTestSuitebuilderClassLibrary"/>
		<rdfs:subClassOf rdf:resource="&android-2_3;AndroidTestSuitebuilderAnnotationClassLibrary"/>
		<rdfs:subClassOf rdf:resource="&android-2_3;AndroidPreferenceClassLibrary"/>
		<rdfs:subClassOf rdf:resource="&android-2_3;AndroidMediaClassLibrary"/>
		<rdfs:subClassOf rdf:resource="&android-2_3;AndroidMediaAudiofxClassLibrary"/>
		<rdfs:subClassOf rdf:resource="&android-2_3;AndroidInputmethodserviceClassLibrary"/>
		<rdfs:subClassOf rdf:resource="&android-2_3;AndroidServiceWallpaperClassLibrary"/>
		<rdfs:subClassOf rdf:resource="&android-2_3;AndroidBluetoothClassLibrary"/>
		<rdfs:subClassOf rdf:resource="&android-2_3;AndroidNfcClassLibrary"/>
		<rdfs:subClassOf rdf:resource="&android-2_3;AndroidProviderClassLibrary"/>
		<rdfs:subClassOf rdf:resource="&android-2_3;AndroidSaxClassLibrary"/>
		<rdfs:subClassOf rdf:resource="&android-2_3;AndroidAppwidgetClassLibrary"/>
		<rdfs:subClassOf rdf:resource="&android-2_3;AndroidOpenglClassLibrary"/>
		<rdfs:subClassOf rdf:resource="&android-2_3;AndroidSpeechClassLibrary"/>
		<rdfs:subClassOf rdf:resource="&android-2_3;AndroidSpeechTtsClassLibrary"/>
		<rdfs:comment xml:lang="en">Java class library implementing the Android 2.3 API</rdfs:comment>
		<rdfs:comment xml:lang="OWLManchester">platform:implementsInterface some Android2_3API</rdfs:comment>
	</owl:Class>
	<owl:Class rdf:about="&android-2_3;Android2_3BytecodeFormat">
		<owl:equivalentClass rdf:resource="&android-2_2;Android2_2BytecodeFormat"/>
		<rdfs:subClassOf rdf:resource="&isa;JavaBytecode"/>
		<rdfs:comment xml:lang="en">Android 2.3 bytecode format</rdfs:comment>
		<rdfs:comment xml:lang="OWLManchester">java:majorVersionNumber some xsd:integer[>="49"^^xsd:integer] and java:preverified value false</rdfs:comment>
	</owl:Class>
	<android-2_3:Android2_3BytecodeFormat rdf:about="&android-2_3;theAndroid2_3BytecodeFormat">
		<java:preverified rdf:datatype="http://www.w3.org/2001/XMLSchema#boolean">false</java:preverified>
		<java:minorVersionNumber rdf:datatype="http://www.w3.org/2001/XMLSchema#integer">0</java:minorVersionNumber>
		<java:majorVersionNumber rdf:datatype="http://www.w3.org/2001/XMLSchema#integer">49</java:majorVersionNumber>
	</android-2_3:Android2_3BytecodeFormat>
	<android-2_3:Android2_3API rdf:about="&android-2_3;theAndroid2_3API">
		<platform:comprisesInterfacePart rdf:resource="&android-2_3;theAndroidSpeechTtsPart"/>
		<platform:comprisesInterfacePart rdf:resource="&android-2_3;theAndroidSpeechPart"/>
		<platform:comprisesInterfacePart rdf:resource="&android-2_3;theAndroidOpenglPart"/>
		<platform:comprisesInterfacePart rdf:resource="&android-2_3;theAndroidAppwidgetPart"/>
		<platform:comprisesInterfacePart rdf:resource="&android-2_3;theAndroidSaxPart"/>
		<platform:comprisesInterfacePart rdf:resource="&android-2_3;theAndroidProviderPart"/>
		<platform:comprisesInterfacePart rdf:resource="&android-2_3;theAndroidNfcPart"/>
		<platform:comprisesInterfacePart rdf:resource="&android-2_3;theAndroidBluetoothPart"/>
		<platform:comprisesInterfacePart rdf:resource="&android-2_3;theAndroidServiceWallpaperPart"/>
		<platform:comprisesInterfacePart rdf:resource="&android-2_3;theAndroidInputmethodservicePart"/>
		<platform:comprisesInterfacePart rdf:resource="&android-2_3;theAndroidMediaAudiofxPart"/>
		<platform:comprisesInterfacePart rdf:resource="&android-2_3;theAndroidMediaPart"/>
		<platform:comprisesInterfacePart rdf:resource="&android-2_3;theAndroidPreferencePart"/>
		<platform:comprisesInterfacePart rdf:resource="&android-2_3;theAndroidTestSuitebuilderAnnotationPart"/>
		<platform:comprisesInterfacePart rdf:resource="&android-2_3;theAndroidTestSuitebuilderPart"/>
		<platform:comprisesInterfacePart rdf:resource="&android-2_3;theAndroidTestMockPart"/>
		<platform:comprisesInterfacePart rdf:resource="&android-2_3;theAndroidTestPart"/>
		<platform:comprisesInterfacePart rdf:resource="&android-2_3;theAndroidWebkitPart"/>
		<platform:comprisesInterfacePart rdf:resource="&android-2_3;theAndroidHardwarePart"/>
		<platform:comprisesInterfacePart rdf:resource="&android-2_3;theAndroidLocationPart"/>
		<platform:comprisesInterfacePart rdf:resource="&android-2_3;theAndroidWidgetPart"/>
		<platform:comprisesInterfacePart rdf:resource="&android-2_3;theAndroidGesturePart"/>
		<platform:comprisesInterfacePart rdf:resource="&android-2_3;theAndroidTextStylePart"/>
		<platform:comprisesInterfacePart rdf:resource="&android-2_3;theAndroidTextMethodPart"/>
		<platform:comprisesInterfacePart rdf:resource="&android-2_3;theAndroidTextFormatPart"/>
		<platform:comprisesInterfacePart rdf:resource="&android-2_3;theAndroidTextUtilPart"/>
		<platform:comprisesInterfacePart rdf:resource="&android-2_3;theAndroidTextPart"/>
		<platform:comprisesInterfacePart rdf:resource="&android-2_3;theAndroidTelephonyGsmPart"/>
		<platform:comprisesInterfacePart rdf:resource="&android-2_3;theAndroidTelephonyCdmaPart"/>
		<platform:comprisesInterfacePart rdf:resource="&android-2_3;theAndroidTelephonyPart"/>
		<platform:comprisesInterfacePart rdf:resource="&android-2_3;theAndroidAppAdminPart"/>
		<platform:comprisesInterfacePart rdf:resource="&android-2_3;theAndroidAppBackupPart"/>
		<platform:comprisesInterfacePart rdf:resource="&android-2_3;theAndroidAppPart"/>
		<platform:comprisesInterfacePart rdf:resource="&android-2_3;theAndroidAccessibilityservicePart"/>
		<platform:comprisesInterfacePart rdf:resource="&android-2_3;theAndroidViewAnimationPart"/>
		<platform:comprisesInterfacePart rdf:resource="&android-2_3;theAndroidViewInputmethodPart"/>
		<platform:comprisesInterfacePart rdf:resource="&android-2_3;theAndroidViewAccessibilityPart"/>
		<platform:comprisesInterfacePart rdf:resource="&android-2_3;theAndroidViewPart"/>
		<platform:comprisesInterfacePart rdf:resource="&android-2_3;theAndroidGraphicsDrawableShapesPart"/>
		<platform:comprisesInterfacePart rdf:resource="&android-2_3;theAndroidGraphicsDrawablePart"/>
		<platform:comprisesInterfacePart rdf:resource="&android-2_3;theAndroidGraphicsPart"/>
		<platform:comprisesInterfacePart rdf:resource="&android-2_3;theAndroidUtilPart"/>
		<platform:comprisesInterfacePart rdf:resource="&android-2_3;theAndroidDatabaseSqlitePart"/>
		<platform:comprisesInterfacePart rdf:resource="&android-2_3;theAndroidDatabasePart"/>
		<platform:comprisesInterfacePart rdf:resource="&android-2_3;theAndroidNetWifiPart"/>
		<platform:comprisesInterfacePart rdf:resource="&android-2_3;theAndroidNetSipPart"/>
		<platform:comprisesInterfacePart rdf:resource="&android-2_3;theAndroidNetHttpPart"/>
		<platform:comprisesInterfacePart rdf:resource="&android-2_3;theAndroidNetPart"/>
		<platform:comprisesInterfacePart rdf:resource="&android-2_3;theAndroidAccountsPart"/>
		<platform:comprisesInterfacePart rdf:resource="&android-2_3;theAndroidOsStoragePart"/>
		<platform:comprisesInterfacePart rdf:resource="&android-2_3;theAndroidOsPart"/>
		<platform:comprisesInterfacePart rdf:resource="&android-2_3;theAndroidContentResPart"/>
		<platform:comprisesInterfacePart rdf:resource="&android-2_3;theAndroidContentPmPart"/>
		<platform:comprisesInterfacePart rdf:resource="&android-2_3;theAndroidContentPart"/>
		<platform:comprisesInterfacePart rdf:resource="&android-2_3;theAndroidPart"/>
		<platform:comprisesInterfacePart rdf:resource="&android-2_3;theJunitFrameworkPart"/>
		<platform:comprisesInterfacePart rdf:resource="&android-2_3;theJunitRunnerPart"/>
		<platform:comprisesInterfacePart rdf:resource="&android-2_3;theDalvikSystemPart"/>
		<platform:comprisesInterfacePart rdf:resource="&android-2_3;theDalvikAnnotationPart"/>
		<platform:comprisesInterfacePart rdf:resource="&android-2_3;theDalvikBytecodePart"/>
		<platform:comprisesInterfacePart rdf:resource="&android-2_3;theOrgJsonPart"/>
		<platform:comprisesInterfacePart rdf:resource="&android-2_3;theOrgApacheCommonsLoggingPart"/>
		<platform:comprisesInterfacePart rdf:resource="&android-2_3;theOrgApacheHttpAuthParamsPart"/>
		<platform:comprisesInterfacePart rdf:resource="&android-2_3;theOrgApacheHttpAuthPart"/>
		<platform:comprisesInterfacePart rdf:resource="&android-2_3;theOrgApacheHttpCookieParamsPart"/>
		<platform:comprisesInterfacePart rdf:resource="&android-2_3;theOrgApacheHttpCookiePart"/>
		<platform:comprisesInterfacePart rdf:resource="&android-2_3;theOrgApacheHttpMessagePart"/>
		<platform:comprisesInterfacePart rdf:resource="&android-2_3;theOrgApacheHttpUtilPart"/>
		<platform:comprisesInterfacePart rdf:resource="&android-2_3;theOrgApacheHttpIoPart"/>
		<platform:comprisesInterfacePart rdf:resource="&android-2_3;theOrgApacheHttpImplClientPart"/>
		<platform:comprisesInterfacePart rdf:resource="&android-2_3;theOrgApacheHttpImplAuthPart"/>
		<platform:comprisesInterfacePart rdf:resource="&android-2_3;theOrgApacheHttpImplCookiePart"/>
		<platform:comprisesInterfacePart rdf:resource="&android-2_3;theOrgApacheHttpImplIoPart"/>
		<platform:comprisesInterfacePart rdf:resource="&android-2_3;theOrgApacheHttpImplConnTsccmPart"/>
		<platform:comprisesInterfacePart rdf:resource="&android-2_3;theOrgApacheHttpImplConnPart"/>
		<platform:comprisesInterfacePart rdf:resource="&android-2_3;theOrgApacheHttpImplEntityPart"/>
		<platform:comprisesInterfacePart rdf:resource="&android-2_3;theOrgApacheHttpImplPart"/>
		<platform:comprisesInterfacePart rdf:resource="&android-2_3;theOrgApacheHttpEntityPart"/>
		<platform:comprisesInterfacePart rdf:resource="&android-2_3;theOrgApacheHttpProtocolPart"/>
		<platform:comprisesInterfacePart rdf:resource="&android-2_3;theOrgApacheHttpConnParamsPart"/>
		<platform:comprisesInterfacePart rdf:resource="&android-2_3;theOrgApacheHttpConnUtilPart"/>
		<platform:comprisesInterfacePart rdf:resource="&android-2_3;theOrgApacheHttpConnSchemePart"/>
		<platform:comprisesInterfacePart rdf:resource="&android-2_3;theOrgApacheHttpConnRoutingPart"/>
		<platform:comprisesInterfacePart rdf:resource="&android-2_3;theOrgApacheHttpConnSslPart"/>
		<platform:comprisesInterfacePart rdf:resource="&android-2_3;theOrgApacheHttpConnPart"/>
		<platform:comprisesInterfacePart rdf:resource="&android-2_3;theOrgApacheHttpParamsPart"/>
		<platform:comprisesInterfacePart rdf:resource="&android-2_3;theOrgApacheHttpClientUtilsPart"/>
		<platform:comprisesInterfacePart rdf:resource="&android-2_3;theOrgApacheHttpClientProtocolPart"/>
		<platform:comprisesInterfacePart rdf:resource="&android-2_3;theOrgApacheHttpClientParamsPart"/>
		<platform:comprisesInterfacePart rdf:resource="&android-2_3;theOrgApacheHttpClientEntityPart"/>
		<platform:comprisesInterfacePart rdf:resource="&android-2_3;theOrgApacheHttpClientMethodsPart"/>
		<platform:comprisesInterfacePart rdf:resource="&android-2_3;theOrgApacheHttpClientPart"/>
		<platform:comprisesInterfacePart rdf:resource="&android-2_3;theOrgApacheHttpPart"/>
		<platform:comprisesInterfacePart rdf:resource="&android-2_3;theOrgXmlpullV1Sax2Part"/>
		<platform:comprisesInterfacePart rdf:resource="&android-2_3;theOrgXmlpullV1Part"/>
		<platform:comprisesInterfacePart rdf:resource="&android-2_3;theOrgW3cDomLsPart"/>
		<platform:comprisesInterfacePart rdf:resource="&android-2_3;theOrgW3cDomPart"/>
		<platform:comprisesInterfacePart rdf:resource="&android-2_3;theOrgXmlSaxHelpersPart"/>
		<platform:comprisesInterfacePart rdf:resource="&android-2_3;theOrgXmlSaxExtPart"/>
		<platform:comprisesInterfacePart rdf:resource="&android-2_3;theOrgXmlSaxPart"/>
		<platform:comprisesInterfacePart rdf:resource="&android-2_3;theJavaAwtFontPart"/>
		<platform:comprisesInterfacePart rdf:resource="&android-2_3;theJavaTextPart"/>
		<platform:comprisesInterfacePart rdf:resource="&android-2_3;theJavaBeansPart"/>
		<platform:comprisesInterfacePart rdf:resource="&android-2_3;theJavaNioCharsetSpiPart"/>
		<platform:comprisesInterfacePart rdf:resource="&android-2_3;theJavaNioCharsetPart"/>
		<platform:comprisesInterfacePart rdf:resource="&android-2_3;theJavaNioChannelsSpiPart"/>
		<platform:comprisesInterfacePart rdf:resource="&android-2_3;theJavaNioChannelsPart"/>
		<platform:comprisesInterfacePart rdf:resource="&android-2_3;theJavaNioPart"/>
		<platform:comprisesInterfacePart rdf:resource="&android-2_3;theJavaSqlPart"/>
		<platform:comprisesInterfacePart rdf:resource="&android-2_3;theJavaSecurityAclPart"/>
		<platform:comprisesInterfacePart rdf:resource="&android-2_3;theJavaSecurityInterfacesPart"/>
		<platform:comprisesInterfacePart rdf:resource="&android-2_3;theJavaSecurityCertPart"/>
		<platform:comprisesInterfacePart rdf:resource="&android-2_3;theJavaSecuritySpecPart"/>
		<platform:comprisesInterfacePart rdf:resource="&android-2_3;theJavaSecurityPart"/>
		<platform:comprisesInterfacePart rdf:resource="&android-2_3;theJavaNetPart"/>
		<platform:comprisesInterfacePart rdf:resource="&android-2_3;theJavaIoPart"/>
		<platform:comprisesInterfacePart rdf:resource="&android-2_3;theJavaMathPart"/>
		<platform:comprisesInterfacePart rdf:resource="&android-2_3;theJavaUtilLoggingPart"/>
		<platform:comprisesInterfacePart rdf:resource="&android-2_3;theJavaUtilConcurrentLocksPart"/>
		<platform:comprisesInterfacePart rdf:resource="&android-2_3;theJavaUtilConcurrentAtomicPart"/>
		<platform:comprisesInterfacePart rdf:resource="&android-2_3;theJavaUtilConcurrentPart"/>
		<platform:comprisesInterfacePart rdf:resource="&android-2_3;theJavaUtilRegexPart"/>
		<platform:comprisesInterfacePart rdf:resource="&android-2_3;theJavaUtilPrefsPart"/>
		<platform:comprisesInterfacePart rdf:resource="&android-2_3;theJavaUtilZipPart"/>
		<platform:comprisesInterfacePart rdf:resource="&android-2_3;theJavaUtilJarPart"/>
		<platform:comprisesInterfacePart rdf:resource="&android-2_3;theJavaUtilPart"/>
		<platform:comprisesInterfacePart rdf:resource="&android-2_3;theJavaLangRefPart"/>
		<platform:comprisesInterfacePart rdf:resource="&android-2_3;theJavaLangAnnotationPart"/>
		<platform:comprisesInterfacePart rdf:resource="&android-2_3;theJavaLangReflectPart"/>
		<platform:comprisesInterfacePart rdf:resource="&android-2_3;theJavaLangPart"/>
		<platform:comprisesInterfacePart rdf:resource="&android-2_3;theJavaxNetSslPart"/>
		<platform:comprisesInterfacePart rdf:resource="&android-2_3;theJavaxNetPart"/>
		<platform:comprisesInterfacePart rdf:resource="&android-2_3;theJavaxMicroeditionKhronosOpenglesPart"/>
		<platform:comprisesInterfacePart rdf:resource="&android-2_3;theJavaxMicroeditionKhronosEglPart"/>
		<platform:comprisesInterfacePart rdf:resource="&android-2_3;theJavaxCryptoSpecPart"/>
		<platform:comprisesInterfacePart rdf:resource="&android-2_3;theJavaxCryptoInterfacesPart"/>
		<platform:comprisesInterfacePart rdf:resource="&android-2_3;theJavaxCryptoPart"/>
		<platform:comprisesInterfacePart rdf:resource="&android-2_3;theJavaxSqlPart"/>
		<platform:comprisesInterfacePart rdf:resource="&android-2_3;theJavaxSecurityAuthX500Part"/>
		<platform:comprisesInterfacePart rdf:resource="&android-2_3;theJavaxSecurityAuthLoginPart"/>
		<platform:comprisesInterfacePart rdf:resource="&android-2_3;theJavaxSecurityAuthCallbackPart"/>
		<platform:comprisesInterfacePart rdf:resource="&android-2_3;theJavaxSecurityAuthPart"/>
		<platform:comprisesInterfacePart rdf:resource="&android-2_3;theJavaxSecurityCertPart"/>
		<platform:comprisesInterfacePart rdf:resource="&android-2_3;theJavaxXmlValidationPart"/>
		<platform:comprisesInterfacePart rdf:resource="&android-2_3;theJavaxXmlParsersPart"/>
		<platform:comprisesInterfacePart rdf:resource="&android-2_3;theJavaxXmlTransformStreamPart"/>
		<platform:comprisesInterfacePart rdf:resource="&android-2_3;theJavaxXmlTransformSaxPart"/>
		<platform:comprisesInterfacePart rdf:resource="&android-2_3;theJavaxXmlTransformDomPart"/>
		<platform:comprisesInterfacePart rdf:resource="&android-2_3;theJavaxXmlTransformPart"/>
		<platform:comprisesInterfacePart rdf:resource="&android-2_3;theJavaxXmlXpathPart"/>
		<platform:comprisesInterfacePart rdf:resource="&android-2_3;theJavaxXmlNamespacePart"/>
		<platform:comprisesInterfacePart rdf:resource="&android-2_3;theJavaxXmlDatatypePart"/>
		<platform:comprisesInterfacePart rdf:resource="&android-2_3;theJavaxXmlPart"/>
	</android-2_3:Android2_3API>
	<owl:Class rdf:about="&android-2_3;Android2_3VM">
		<owl:equivalentClass>
			<owl:Restriction>
				<owl:onProperty rdf:resource="&platform;implementsInterface"/>
				<owl:someValuesFrom rdf:resource="&android-2_3;Android2_3BytecodeFormat"/>
			</owl:Restriction>
		</owl:equivalentClass>
		<rdfs:subClassOf rdf:resource="&java;JavaVM"/>
		<rdfs:comment xml:lang="en">Android 2.3 virtual machine</rdfs:comment>
	</owl:Class>
	<owl:Class rdf:about="&android-2_3;Android2_3JRE">
		<owl:equivalentClass>
			<owl:Class >
				<owl:intersectionOf rdf:parseType="Collection">
					<owl:Restriction>
						<owl:onProperty rdf:resource="&platform;providesFeature"/>
						<owl:someValuesFrom rdf:resource="&android-2_3;Android2_3ClassLibrary"/>
					</owl:Restriction>
					<owl:Restriction>
						<owl:onProperty rdf:resource="&platform;providesFeature"/>
						<owl:someValuesFrom rdf:resource="&android-2_3;Android2_3VM"/>
					</owl:Restriction>
				</owl:intersectionOf>
			</owl:Class>
		</owl:equivalentClass>
		<rdfs:subClassOf rdf:resource="&java;JRE"/>
		<rdfs:comment xml:lang="en">Android 2.3 Java Runtime Environment</rdfs:comment>
	</owl:Class>
	<owl:Class rdf:about="&android-2_3;JavaxXml">
		<owl:equivalentClass rdf:resource="&java-se-6;JavaxXml"/>
		<owl:equivalentClass rdf:resource="&android-2_2;JavaxXml"/>
		<rdfs:subClassOf rdf:resource="&java;JavaAPIPart"/>
		<rdfs:seeAlso rdf:resource="&android-2_3;JavaLang"/>
		<rdfs:comment xml:lang="en">Java API part implementing the javax.xml package for Android 2.3</rdfs:comment>
	</owl:Class>
	<owl:Class rdf:about="&android-2_3;JavaxXmlDatatype">
		<owl:equivalentClass rdf:resource="&java-se-6;JavaxXmlDatatype"/>
		<rdfs:subClassOf rdf:resource="&android-2_2;JavaxXmlDatatype"/>
		<rdfs:seeAlso rdf:resource="&android-2_3;JavaxXmlNamespace"/>
		<rdfs:seeAlso rdf:resource="&android-2_3;JavaIo"/>
		<rdfs:seeAlso rdf:resource="&android-2_3;JavaLang"/>
		<rdfs:seeAlso rdf:resource="&android-2_3;JavaUtil"/>
		<rdfs:seeAlso rdf:resource="&android-2_3;JavaMath"/>
		<rdfs:comment xml:lang="en">Java API part implementing the javax.xml.datatype package for Android 2.3</rdfs:comment>
	</owl:Class>
	<owl:Class rdf:about="&android-2_3;JavaxXmlNamespace">
		<owl:equivalentClass rdf:resource="&java-se-6;JavaxXmlNamespace"/>
		<owl:equivalentClass rdf:resource="&android-2_2;JavaxXmlNamespace"/>
		<rdfs:subClassOf rdf:resource="&java;JavaAPIPart"/>
		<rdfs:seeAlso rdf:resource="&android-2_3;JavaUtil"/>
		<rdfs:seeAlso rdf:resource="&android-2_3;JavaIo"/>
		<rdfs:seeAlso rdf:resource="&android-2_3;JavaLang"/>
		<rdfs:comment xml:lang="en">Java API part implementing the javax.xml.namespace package for Android 2.3</rdfs:comment>
	</owl:Class>
	<owl:Class rdf:about="&android-2_3;JavaxXmlXpath">
		<owl:equivalentClass rdf:resource="&java-se-6;JavaxXmlXpath"/>
		<owl:equivalentClass rdf:resource="&android-2_2;JavaxXmlXpath"/>
		<rdfs:subClassOf rdf:resource="&java;JavaAPIPart"/>
		<rdfs:seeAlso rdf:resource="&android-2_3;OrgXmlSax"/>
		<rdfs:seeAlso rdf:resource="&android-2_3;JavaxXmlNamespace"/>
		<rdfs:seeAlso rdf:resource="&android-2_3;JavaUtil"/>
		<rdfs:seeAlso rdf:resource="&android-2_3;JavaIo"/>
		<rdfs:seeAlso rdf:resource="&android-2_3;JavaLang"/>
		<rdfs:comment xml:lang="en">Java API part implementing the javax.xml.xpath package for Android 2.3</rdfs:comment>
	</owl:Class>
	<owl:Class rdf:about="&android-2_3;JavaxXmlTransform">
		<owl:equivalentClass rdf:resource="&java-se-6;JavaxXmlTransform"/>
		<rdfs:subClassOf rdf:resource="&android-2_2;JavaxXmlTransform"/>
		<rdfs:seeAlso rdf:resource="&android-2_3;JavaUtil"/>
		<rdfs:seeAlso rdf:resource="&android-2_3;JavaIo"/>
		<rdfs:seeAlso rdf:resource="&android-2_3;JavaLang"/>
		<rdfs:comment xml:lang="en">Java API part implementing the javax.xml.transform package for Android 2.3</rdfs:comment>
	</owl:Class>
	<owl:Class rdf:about="&android-2_3;JavaxXmlTransformDom">
		<owl:equivalentClass rdf:resource="&java-se-6;JavaxXmlTransformDom"/>
		<owl:equivalentClass rdf:resource="&android-2_2;JavaxXmlTransformDom"/>
		<rdfs:subClassOf rdf:resource="&java;JavaAPIPart"/>
		<rdfs:seeAlso rdf:resource="&android-2_3;JavaxXmlTransform"/>
		<rdfs:seeAlso rdf:resource="&android-2_3;JavaLang"/>
		<rdfs:seeAlso rdf:resource="&android-2_3;OrgW3cDom"/>
		<rdfs:comment xml:lang="en">Java API part implementing the javax.xml.transform.dom package for Android 2.3</rdfs:comment>
	</owl:Class>
	<owl:Class rdf:about="&android-2_3;JavaxXmlTransformSax">
		<owl:equivalentClass rdf:resource="&java-se-6;JavaxXmlTransformSax"/>
		<rdfs:subClassOf rdf:resource="&android-2_2;JavaxXmlTransformSax"/>
		<rdfs:seeAlso rdf:resource="&android-2_3;OrgXmlSax"/>
		<rdfs:seeAlso rdf:resource="&android-2_3;OrgXmlSaxExt"/>
		<rdfs:seeAlso rdf:resource="&android-2_3;JavaLang"/>
		<rdfs:seeAlso rdf:resource="&android-2_3;JavaxXmlTransform"/>
		<rdfs:comment xml:lang="en">Java API part implementing the javax.xml.transform.sax package for Android 2.3</rdfs:comment>
	</owl:Class>
	<owl:Class rdf:about="&android-2_3;JavaxXmlTransformStream">
		<owl:equivalentClass rdf:resource="&java-se-6;JavaxXmlTransformStream"/>
		<owl:equivalentClass rdf:resource="&android-2_2;JavaxXmlTransformStream"/>
		<rdfs:subClassOf rdf:resource="&java;JavaAPIPart"/>
		<rdfs:seeAlso rdf:resource="&android-2_3;JavaxXmlTransform"/>
		<rdfs:seeAlso rdf:resource="&android-2_3;JavaIo"/>
		<rdfs:seeAlso rdf:resource="&android-2_3;JavaLang"/>
		<rdfs:comment xml:lang="en">Java API part implementing the javax.xml.transform.stream package for Android 2.3</rdfs:comment>
	</owl:Class>
	<owl:Class rdf:about="&android-2_3;JavaxXmlParsers">
		<owl:equivalentClass rdf:resource="&java-se-6;JavaxXmlParsers"/>
		<rdfs:subClassOf rdf:resource="&android-2_2;JavaxXmlParsers"/>
		<rdfs:seeAlso rdf:resource="&android-2_3;OrgXmlSax"/>
		<rdfs:seeAlso rdf:resource="&android-2_3;OrgXmlSaxHelpers"/>
		<rdfs:seeAlso rdf:resource="&android-2_3;JavaIo"/>
		<rdfs:seeAlso rdf:resource="&android-2_3;JavaLang"/>
		<rdfs:seeAlso rdf:resource="&android-2_3;JavaxXmlValidation"/>
		<rdfs:seeAlso rdf:resource="&android-2_3;OrgW3cDom"/>
		<rdfs:comment xml:lang="en">Java API part implementing the javax.xml.parsers package for Android 2.3</rdfs:comment>
	</owl:Class>
	<owl:Class rdf:about="&android-2_3;JavaxXmlValidation">
		<rdfs:subClassOf rdf:resource="&java-se-6;JavaxXmlValidation"/>
		<rdfs:subClassOf rdf:resource="&android-2_2;JavaxXmlValidation"/>
		<rdfs:seeAlso rdf:resource="&android-2_3;JavaNet"/>
		<rdfs:seeAlso rdf:resource="&android-2_3;OrgXmlSax"/>
		<rdfs:seeAlso rdf:resource="&android-2_3;OrgW3cDomLs"/>
		<rdfs:seeAlso rdf:resource="&android-2_3;JavaIo"/>
		<rdfs:seeAlso rdf:resource="&android-2_3;JavaxXmlTransform"/>
		<rdfs:seeAlso rdf:resource="&android-2_3;JavaLang"/>
		<rdfs:seeAlso rdf:resource="&android-2_3;OrgW3cDom"/>
		<rdfs:comment xml:lang="en">Java API part implementing the javax.xml.validation package for Android 2.3</rdfs:comment>
	</owl:Class>
	<owl:Class rdf:about="&android-2_3;JavaxSecurityCert">
		<owl:equivalentClass rdf:resource="&java-se-6;JavaxSecurityCert"/>
		<owl:equivalentClass rdf:resource="&android-2_2;JavaxSecurityCert"/>
		<rdfs:subClassOf rdf:resource="&java;JavaAPIPart"/>
		<rdfs:seeAlso rdf:resource="&android-2_3;JavaSecurity"/>
		<rdfs:seeAlso rdf:resource="&android-2_3;JavaUtil"/>
		<rdfs:seeAlso rdf:resource="&android-2_3;JavaIo"/>
		<rdfs:seeAlso rdf:resource="&android-2_3;JavaLang"/>
		<rdfs:seeAlso rdf:resource="&android-2_3;JavaMath"/>
		<rdfs:comment xml:lang="en">Java API part implementing the javax.security.cert package for Android 2.3</rdfs:comment>
	</owl:Class>
	<owl:Class rdf:about="&android-2_3;JavaxSecurityAuth">
		<owl:equivalentClass rdf:resource="&android-2_2;JavaxSecurityAuth"/>
		<rdfs:subClassOf rdf:resource="&java;JavaAPIPart"/>
		<rdfs:seeAlso rdf:resource="&android-2_3;JavaSecurity"/>
		<rdfs:seeAlso rdf:resource="&android-2_3;JavaIo"/>
		<rdfs:seeAlso rdf:resource="&android-2_3;JavaLang"/>
		<rdfs:seeAlso rdf:resource="&android-2_3;JavaUtil"/>
		<rdfs:comment xml:lang="en">Java API part implementing the javax.security.auth package for Android 2.3</rdfs:comment>
	</owl:Class>
	<owl:Class rdf:about="&android-2_3;JavaxSecurityAuthCallback">
		<owl:equivalentClass rdf:resource="&android-2_2;JavaxSecurityAuthCallback"/>
		<rdfs:subClassOf rdf:resource="&java;JavaAPIPart"/>
		<rdfs:seeAlso rdf:resource="&android-2_3;JavaIo"/>
		<rdfs:seeAlso rdf:resource="&android-2_3;JavaLang"/>
		<rdfs:comment xml:lang="en">Java API part implementing the javax.security.auth.callback package for Android 2.3</rdfs:comment>
	</owl:Class>
	<owl:Class rdf:about="&android-2_3;JavaxSecurityAuthLogin">
		<owl:equivalentClass rdf:resource="&android-2_2;JavaxSecurityAuthLogin"/>
		<rdfs:subClassOf rdf:resource="&java;JavaAPIPart"/>
		<rdfs:seeAlso rdf:resource="&android-2_3;JavaSecurity"/>
		<rdfs:seeAlso rdf:resource="&android-2_3;JavaLang"/>
		<rdfs:comment xml:lang="en">Java API part implementing the javax.security.auth.login package for Android 2.3</rdfs:comment>
	</owl:Class>
	<owl:Class rdf:about="&android-2_3;JavaxSecurityAuthX500">
		<rdfs:subClassOf rdf:resource="&android-2_2;JavaxSecurityAuthX500"/>
		<rdfs:seeAlso rdf:resource="&android-2_3;JavaSecurity"/>
		<rdfs:seeAlso rdf:resource="&android-2_3;JavaUtil"/>
		<rdfs:seeAlso rdf:resource="&android-2_3;JavaIo"/>
		<rdfs:seeAlso rdf:resource="&android-2_3;JavaLang"/>
		<rdfs:comment xml:lang="en">Java API part implementing the javax.security.auth.x500 package for Android 2.3</rdfs:comment>
	</owl:Class>
	<owl:Class rdf:about="&android-2_3;JavaxSql">
		<rdfs:subClassOf rdf:resource="&android-2_2;JavaxSql"/>
		<rdfs:seeAlso rdf:resource="&android-2_3;JavaSql"/>
		<rdfs:seeAlso rdf:resource="&android-2_3;JavaIo"/>
		<rdfs:seeAlso rdf:resource="&android-2_3;JavaLang"/>
		<rdfs:seeAlso rdf:resource="&android-2_3;JavaNet"/>
		<rdfs:seeAlso rdf:resource="&android-2_3;JavaUtil"/>
		<rdfs:seeAlso rdf:resource="&android-2_3;JavaMath"/>
		<rdfs:comment xml:lang="en">Java API part implementing the javax.sql package for Android 2.3</rdfs:comment>
	</owl:Class>
	<owl:Class rdf:about="&android-2_3;JavaxCrypto">
		<owl:equivalentClass rdf:resource="&java-se-6;JavaxCrypto"/>
		<owl:equivalentClass rdf:resource="&android-2_2;JavaxCrypto"/>
		<rdfs:subClassOf rdf:resource="&java;JavaAPIPart"/>
		<rdfs:seeAlso rdf:resource="&android-2_3;JavaSecurity"/>
		<rdfs:seeAlso rdf:resource="&android-2_3;JavaSecuritySpec"/>
		<rdfs:seeAlso rdf:resource="&android-2_3;JavaIo"/>
		<rdfs:seeAlso rdf:resource="&android-2_3;JavaLang"/>
		<rdfs:seeAlso rdf:resource="&android-2_3;JavaSecurityCert"/>
		<rdfs:seeAlso rdf:resource="&android-2_3;JavaNio"/>
		<rdfs:comment xml:lang="en">Java API part implementing the javax.crypto package for Android 2.3</rdfs:comment>
	</owl:Class>
	<owl:Class rdf:about="&android-2_3;JavaxCryptoInterfaces">
		<owl:equivalentClass rdf:resource="&java-se-6;JavaxCryptoInterfaces"/>
		<owl:equivalentClass rdf:resource="&android-2_2;JavaxCryptoInterfaces"/>
		<rdfs:subClassOf rdf:resource="&java;JavaAPIPart"/>
		<rdfs:seeAlso rdf:resource="&android-2_3;JavaSecurity"/>
		<rdfs:seeAlso rdf:resource="&android-2_3;JavaxCryptoSpec"/>
		<rdfs:seeAlso rdf:resource="&android-2_3;JavaxCrypto"/>
		<rdfs:seeAlso rdf:resource="&android-2_3;JavaMath"/>
		<rdfs:comment xml:lang="en">Java API part implementing the javax.crypto.interfaces package for Android 2.3</rdfs:comment>
	</owl:Class>
	<owl:Class rdf:about="&android-2_3;JavaxCryptoSpec">
		<owl:equivalentClass rdf:resource="&java-se-6;JavaxCryptoSpec"/>
		<owl:equivalentClass rdf:resource="&android-2_2;JavaxCryptoSpec"/>
		<rdfs:subClassOf rdf:resource="&java;JavaAPIPart"/>
		<rdfs:seeAlso rdf:resource="&android-2_3;JavaxCrypto"/>
		<rdfs:seeAlso rdf:resource="&android-2_3;JavaSecuritySpec"/>
		<rdfs:seeAlso rdf:resource="&android-2_3;JavaIo"/>
		<rdfs:seeAlso rdf:resource="&android-2_3;JavaLang"/>
		<rdfs:seeAlso rdf:resource="&android-2_3;JavaMath"/>
		<rdfs:comment xml:lang="en">Java API part implementing the javax.crypto.spec package for Android 2.3</rdfs:comment>
	</owl:Class>
	<owl:Class rdf:about="&android-2_3;JavaxMicroeditionKhronosEgl">
		<owl:equivalentClass rdf:resource="&android-2_2;JavaxMicroeditionKhronosEgl"/>
		<rdfs:subClassOf rdf:resource="&java;JavaAPIPart"/>
		<rdfs:seeAlso rdf:resource="&android-2_3;JavaLang"/>
		<rdfs:seeAlso rdf:resource="&android-2_3;JavaxMicroeditionKhronosOpengles"/>
		<rdfs:comment xml:lang="en">Java API part implementing the javax.microedition.khronos.egl package for Android 2.3</rdfs:comment>
	</owl:Class>
	<owl:Class rdf:about="&android-2_3;JavaxMicroeditionKhronosOpengles">
		<owl:equivalentClass rdf:resource="&android-2_2;JavaxMicroeditionKhronosOpengles"/>
		<rdfs:subClassOf rdf:resource="&java;JavaAPIPart"/>
		<rdfs:seeAlso rdf:resource="&android-2_3;JavaLang"/>
		<rdfs:seeAlso rdf:resource="&android-2_3;JavaNio"/>
		<rdfs:comment xml:lang="en">Java API part implementing the javax.microedition.khronos.opengles package for Android 2.3</rdfs:comment>
	</owl:Class>
	<owl:Class rdf:about="&android-2_3;JavaxNet">
		<owl:equivalentClass rdf:resource="&java-se-6;JavaxNet"/>
		<owl:equivalentClass rdf:resource="&android-2_2;JavaxNet"/>
		<rdfs:subClassOf rdf:resource="&java;JavaAPIPart"/>
		<rdfs:seeAlso rdf:resource="&android-2_3;JavaNet"/>
		<rdfs:seeAlso rdf:resource="&android-2_3;JavaLang"/>
		<rdfs:comment xml:lang="en">Java API part implementing the javax.net package for Android 2.3</rdfs:comment>
	</owl:Class>
	<owl:Class rdf:about="&android-2_3;JavaxNetSsl">
		<owl:equivalentClass rdf:resource="&java-se-6;JavaxNetSsl"/>
		<rdfs:subClassOf rdf:resource="&android-2_2;JavaxNetSsl"/>
		<rdfs:seeAlso rdf:resource="&android-2_3;JavaSecurityCert"/>
		<rdfs:seeAlso rdf:resource="&android-2_3;JavaNio"/>
		<rdfs:seeAlso rdf:resource="&android-2_3;JavaSecurity"/>
		<rdfs:seeAlso rdf:resource="&android-2_3;JavaIo"/>
		<rdfs:seeAlso rdf:resource="&android-2_3;JavaLang"/>
		<rdfs:seeAlso rdf:resource="&android-2_3;JavaNet"/>
		<rdfs:seeAlso rdf:resource="&android-2_3;JavaxNet"/>
		<rdfs:seeAlso rdf:resource="&android-2_3;JavaUtil"/>
		<rdfs:comment xml:lang="en">Java API part implementing the javax.net.ssl package for Android 2.3</rdfs:comment>
	</owl:Class>
	<owl:Class rdf:about="&android-2_3;JavaLang">
		<rdfs:subClassOf rdf:resource="&java;JavaAPIPart"/>
		<rdfs:seeAlso rdf:resource="&android-2_3;JavaNioCharset"/>
		<rdfs:seeAlso rdf:resource="&android-2_3;JavaNio"/>
		<rdfs:seeAlso rdf:resource="&android-2_3;JavaNioChannels"/>
		<rdfs:seeAlso rdf:resource="&android-2_3;JavaLangReflect"/>
		<rdfs:seeAlso rdf:resource="&android-2_3;JavaSecurity"/>
		<rdfs:seeAlso rdf:resource="&android-2_3;JavaIo"/>
		<rdfs:seeAlso rdf:resource="&android-2_3;JavaLangAnnotation"/>
		<rdfs:seeAlso rdf:resource="&android-2_3;JavaNet"/>
		<rdfs:seeAlso rdf:resource="&android-2_3;JavaUtil"/>
		<rdfs:comment xml:lang="en">Java API part implementing the java.lang package for Android 2.3</rdfs:comment>
	</owl:Class>
	<owl:Class rdf:about="&android-2_3;JavaLangReflect">
		<owl:equivalentClass rdf:resource="&java-se-6;JavaLangReflect"/>
		<owl:equivalentClass rdf:resource="&android-2_2;JavaLangReflect"/>
		<rdfs:subClassOf rdf:resource="&java;JavaAPIPart"/>
		<rdfs:seeAlso rdf:resource="&android-2_3;JavaSecurity"/>
		<rdfs:seeAlso rdf:resource="&android-2_3;JavaIo"/>
		<rdfs:seeAlso rdf:resource="&android-2_3;JavaLang"/>
		<rdfs:seeAlso rdf:resource="&android-2_3;JavaLangAnnotation"/>
		<rdfs:comment xml:lang="en">Java API part implementing the java.lang.reflect package for Android 2.3</rdfs:comment>
	</owl:Class>
	<owl:Class rdf:about="&android-2_3;JavaLangAnnotation">
		<owl:equivalentClass rdf:resource="&java-se-6;JavaLangAnnotation"/>
		<rdfs:subClassOf rdf:resource="&android-2_2;JavaLangAnnotation"/>
		<rdfs:seeAlso rdf:resource="&android-2_3;JavaLangReflect"/>
		<rdfs:seeAlso rdf:resource="&android-2_3;JavaLang"/>
		<rdfs:comment xml:lang="en">Java API part implementing the java.lang.annotation package for Android 2.3</rdfs:comment>
	</owl:Class>
	<owl:Class rdf:about="&android-2_3;JavaLangRef">
		<owl:equivalentClass rdf:resource="&java-se-6;JavaLangRef"/>
		<owl:equivalentClass rdf:resource="&android-2_2;JavaLangRef"/>
		<rdfs:subClassOf rdf:resource="&java;JavaAPIPart"/>
		<rdfs:seeAlso rdf:resource="&android-2_3;JavaLang"/>
		<rdfs:comment xml:lang="en">Java API part implementing the java.lang.ref package for Android 2.3</rdfs:comment>
	</owl:Class>
	<owl:Class rdf:about="&android-2_3;JavaUtil">
		<owl:equivalentClass rdf:resource="&java-se-6;JavaUtil"/>
		<rdfs:subClassOf rdf:resource="&android-2_2;JavaUtil"/>
		<rdfs:seeAlso rdf:resource="&android-2_3;JavaNioChannels"/>
		<rdfs:seeAlso rdf:resource="&android-2_3;JavaSecurity"/>
		<rdfs:seeAlso rdf:resource="&android-2_3;JavaUtilRegex"/>
		<rdfs:seeAlso rdf:resource="&android-2_3;JavaIo"/>
		<rdfs:seeAlso rdf:resource="&android-2_3;JavaLang"/>
		<rdfs:seeAlso rdf:resource="&android-2_3;JavaMath"/>
		<rdfs:comment xml:lang="en">Java API part implementing the java.util package for Android 2.3</rdfs:comment>
	</owl:Class>
	<owl:Class rdf:about="&android-2_3;JavaUtilJar">
		<owl:equivalentClass rdf:resource="&java-se-6;JavaUtilJar"/>
		<owl:equivalentClass rdf:resource="&android-2_2;JavaUtilJar"/>
		<rdfs:subClassOf rdf:resource="&java;JavaAPIPart"/>
		<rdfs:seeAlso rdf:resource="&android-2_3;JavaUtilZip"/>
		<rdfs:seeAlso rdf:resource="&android-2_3;JavaIo"/>
		<rdfs:seeAlso rdf:resource="&android-2_3;JavaLang"/>
		<rdfs:seeAlso rdf:resource="&android-2_3;JavaBeans"/>
		<rdfs:seeAlso rdf:resource="&android-2_3;JavaUtil"/>
		<rdfs:comment xml:lang="en">Java API part implementing the java.util.jar package for Android 2.3</rdfs:comment>
	</owl:Class>
	<owl:Class rdf:about="&android-2_3;JavaUtilZip">
		<owl:equivalentClass rdf:resource="&java-se-6;JavaUtilZip"/>
		<rdfs:subClassOf rdf:resource="&android-2_2;JavaUtilZip"/>
		<rdfs:seeAlso rdf:resource="&android-2_3;JavaIo"/>
		<rdfs:seeAlso rdf:resource="&android-2_3;JavaLang"/>
		<rdfs:seeAlso rdf:resource="&android-2_3;JavaUtil"/>
		<rdfs:comment xml:lang="en">Java API part implementing the java.util.zip package for Android 2.3</rdfs:comment>
	</owl:Class>
	<owl:Class rdf:about="&android-2_3;JavaUtilPrefs">
		<owl:equivalentClass rdf:resource="&java-se-6;JavaUtilPrefs"/>
		<owl:equivalentClass rdf:resource="&android-2_2;JavaUtilPrefs"/>
		<rdfs:subClassOf rdf:resource="&java;JavaAPIPart"/>
		<rdfs:seeAlso rdf:resource="&android-2_3;JavaUtil"/>
		<rdfs:seeAlso rdf:resource="&android-2_3;JavaIo"/>
		<rdfs:seeAlso rdf:resource="&android-2_3;JavaLang"/>
		<rdfs:comment xml:lang="en">Java API part implementing the java.util.prefs package for Android 2.3</rdfs:comment>
	</owl:Class>
	<owl:Class rdf:about="&android-2_3;JavaUtilRegex">
		<owl:equivalentClass rdf:resource="&java-se-6;JavaUtilRegex"/>
		<owl:equivalentClass rdf:resource="&android-2_2;JavaUtilRegex"/>
		<rdfs:subClassOf rdf:resource="&java;JavaAPIPart"/>
		<rdfs:seeAlso rdf:resource="&android-2_3;JavaIo"/>
		<rdfs:seeAlso rdf:resource="&android-2_3;JavaLang"/>
		<rdfs:comment xml:lang="en">Java API part implementing the java.util.regex package for Android 2.3</rdfs:comment>
	</owl:Class>
	<owl:Class rdf:about="&android-2_3;JavaUtilConcurrent">
		<rdfs:subClassOf rdf:resource="&android-2_2;JavaUtilConcurrent"/>
		<rdfs:seeAlso rdf:resource="&android-2_3;JavaSecurity"/>
		<rdfs:seeAlso rdf:resource="&android-2_3;JavaIo"/>
		<rdfs:seeAlso rdf:resource="&android-2_3;JavaLang"/>
		<rdfs:seeAlso rdf:resource="&android-2_3;JavaUtil"/>
		<rdfs:comment xml:lang="en">Java API part implementing the java.util.concurrent package for Android 2.3</rdfs:comment>
	</owl:Class>
	<owl:Class rdf:about="&android-2_3;JavaUtilConcurrentAtomic">
		<owl:equivalentClass rdf:resource="&java-se-6;JavaUtilConcurrentAtomic"/>
		<rdfs:subClassOf rdf:resource="&android-2_2;JavaUtilConcurrentAtomic"/>
		<rdfs:seeAlso rdf:resource="&android-2_3;JavaIo"/>
		<rdfs:seeAlso rdf:resource="&android-2_3;JavaLang"/>
		<rdfs:comment xml:lang="en">Java API part implementing the java.util.concurrent.atomic package for Android 2.3</rdfs:comment>
	</owl:Class>
	<owl:Class rdf:about="&android-2_3;JavaUtilConcurrentLocks">
		<owl:equivalentClass rdf:resource="&java-se-6;JavaUtilConcurrentLocks"/>
		<rdfs:subClassOf rdf:resource="&android-2_2;JavaUtilConcurrentLocks"/>
		<rdfs:seeAlso rdf:resource="&android-2_3;JavaUtilConcurrent"/>
		<rdfs:seeAlso rdf:resource="&android-2_3;JavaUtil"/>
		<rdfs:seeAlso rdf:resource="&android-2_3;JavaIo"/>
		<rdfs:seeAlso rdf:resource="&android-2_3;JavaLang"/>
		<rdfs:comment xml:lang="en">Java API part implementing the java.util.concurrent.locks package for Android 2.3</rdfs:comment>
	</owl:Class>
	<owl:Class rdf:about="&android-2_3;JavaUtilLogging">
		<owl:equivalentClass rdf:resource="&java-se-6;JavaUtilLogging"/>
		<rdfs:subClassOf rdf:resource="&android-2_2;JavaUtilLogging"/>
		<rdfs:seeAlso rdf:resource="&android-2_3;JavaSecurity"/>
		<rdfs:seeAlso rdf:resource="&android-2_3;JavaIo"/>
		<rdfs:seeAlso rdf:resource="&android-2_3;JavaLang"/>
		<rdfs:seeAlso rdf:resource="&android-2_3;JavaBeans"/>
		<rdfs:seeAlso rdf:resource="&android-2_3;JavaUtil"/>
		<rdfs:comment xml:lang="en">Java API part implementing the java.util.logging package for Android 2.3</rdfs:comment>
	</owl:Class>
	<owl:Class rdf:about="&android-2_3;JavaMath">
		<owl:equivalentClass rdf:resource="&java-se-6;JavaMath"/>
		<rdfs:subClassOf rdf:resource="&android-2_2;JavaMath"/>
		<rdfs:seeAlso rdf:resource="&android-2_3;JavaUtil"/>
		<rdfs:seeAlso rdf:resource="&android-2_3;JavaIo"/>
		<rdfs:seeAlso rdf:resource="&android-2_3;JavaLang"/>
		<rdfs:comment xml:lang="en">Java API part implementing the java.math package for Android 2.3</rdfs:comment>
	</owl:Class>
	<owl:Class rdf:about="&android-2_3;JavaIo">
		<owl:equivalentClass rdf:resource="&java-se-6;JavaIo"/>
		<rdfs:subClassOf rdf:resource="&android-2_2;JavaIo"/>
		<rdfs:seeAlso rdf:resource="&android-2_3;JavaSecurity"/>
		<rdfs:seeAlso rdf:resource="&android-2_3;JavaNioCharset"/>
		<rdfs:seeAlso rdf:resource="&android-2_3;JavaLang"/>
		<rdfs:seeAlso rdf:resource="&android-2_3;JavaNio"/>
		<rdfs:seeAlso rdf:resource="&android-2_3;JavaNet"/>
		<rdfs:seeAlso rdf:resource="&android-2_3;JavaNioChannels"/>
		<rdfs:seeAlso rdf:resource="&android-2_3;JavaUtil"/>
		<rdfs:comment xml:lang="en">Java API part implementing the java.io package for Android 2.3</rdfs:comment>
	</owl:Class>
	<owl:Class rdf:about="&android-2_3;JavaNet">
		<owl:equivalentClass rdf:resource="&java-se-6;JavaNet"/>
		<rdfs:subClassOf rdf:resource="&android-2_2;JavaNet"/>
		<rdfs:seeAlso rdf:resource="&android-2_3;JavaNioChannels"/>
		<rdfs:seeAlso rdf:resource="&android-2_3;JavaUtilJar"/>
		<rdfs:seeAlso rdf:resource="&android-2_3;JavaSecurity"/>
		<rdfs:seeAlso rdf:resource="&android-2_3;JavaIo"/>
		<rdfs:seeAlso rdf:resource="&android-2_3;JavaLang"/>
		<rdfs:seeAlso rdf:resource="&android-2_3;JavaUtil"/>
		<rdfs:comment xml:lang="en">Java API part implementing the java.net package for Android 2.3</rdfs:comment>
	</owl:Class>
	<owl:Class rdf:about="&android-2_3;JavaSecurity">
		<rdfs:subClassOf rdf:resource="&android-2_2;JavaSecurity"/>
		<rdfs:seeAlso rdf:resource="&android-2_3;JavaxCrypto"/>
		<rdfs:seeAlso rdf:resource="&android-2_3;JavaSecurityCert"/>
		<rdfs:seeAlso rdf:resource="&android-2_3;JavaNio"/>
		<rdfs:seeAlso rdf:resource="&android-2_3;JavaSecuritySpec"/>
		<rdfs:seeAlso rdf:resource="&android-2_3;JavaIo"/>
		<rdfs:seeAlso rdf:resource="&android-2_3;JavaLang"/>
		<rdfs:seeAlso rdf:resource="&android-2_3;JavaNet"/>
		<rdfs:seeAlso rdf:resource="&android-2_3;JavaxSecurityAuthCallback"/>
		<rdfs:seeAlso rdf:resource="&android-2_3;JavaUtil"/>
		<rdfs:seeAlso rdf:resource="&android-2_3;JavaxSecurityAuth"/>
		<rdfs:comment xml:lang="en">Java API part implementing the java.security package for Android 2.3</rdfs:comment>
	</owl:Class>
	<owl:Class rdf:about="&android-2_3;JavaSecuritySpec">
		<owl:equivalentClass rdf:resource="&java-se-6;JavaSecuritySpec"/>
		<owl:equivalentClass rdf:resource="&android-2_2;JavaSecuritySpec"/>
		<rdfs:subClassOf rdf:resource="&java;JavaAPIPart"/>
		<rdfs:seeAlso rdf:resource="&android-2_3;JavaSecurity"/>
		<rdfs:seeAlso rdf:resource="&android-2_3;JavaSecurityInterfaces"/>
		<rdfs:seeAlso rdf:resource="&android-2_3;JavaLang"/>
		<rdfs:seeAlso rdf:resource="&android-2_3;JavaMath"/>
		<rdfs:comment xml:lang="en">Java API part implementing the java.security.spec package for Android 2.3</rdfs:comment>
	</owl:Class>
	<owl:Class rdf:about="&android-2_3;JavaSecurityCert">
		<owl:equivalentClass rdf:resource="&java-se-6;JavaSecurityCert"/>
		<owl:equivalentClass rdf:resource="&android-2_2;JavaSecurityCert"/>
		<rdfs:subClassOf rdf:resource="&java;JavaAPIPart"/>
		<rdfs:seeAlso rdf:resource="&android-2_3;JavaSecurity"/>
		<rdfs:seeAlso rdf:resource="&android-2_3;JavaIo"/>
		<rdfs:seeAlso rdf:resource="&android-2_3;JavaLang"/>
		<rdfs:seeAlso rdf:resource="&android-2_3;JavaUtil"/>
		<rdfs:seeAlso rdf:resource="&android-2_3;JavaxSecurityAuthX500"/>
		<rdfs:seeAlso rdf:resource="&android-2_3;JavaMath"/>
		<rdfs:comment xml:lang="en">Java API part implementing the java.security.cert package for Android 2.3</rdfs:comment>
	</owl:Class>
	<owl:Class rdf:about="&android-2_3;JavaSecurityInterfaces">
		<owl:equivalentClass rdf:resource="&java-se-6;JavaSecurityInterfaces"/>
		<owl:equivalentClass rdf:resource="&android-2_2;JavaSecurityInterfaces"/>
		<rdfs:subClassOf rdf:resource="&java;JavaAPIPart"/>
		<rdfs:seeAlso rdf:resource="&android-2_3;JavaSecurity"/>
		<rdfs:seeAlso rdf:resource="&android-2_3;JavaSecuritySpec"/>
		<rdfs:seeAlso rdf:resource="&android-2_3;JavaMath"/>
		<rdfs:comment xml:lang="en">Java API part implementing the java.security.interfaces package for Android 2.3</rdfs:comment>
	</owl:Class>
	<owl:Class rdf:about="&android-2_3;JavaSecurityAcl">
		<owl:equivalentClass rdf:resource="&java-se-6;JavaSecurityAcl"/>
		<owl:equivalentClass rdf:resource="&android-2_2;JavaSecurityAcl"/>
		<rdfs:subClassOf rdf:resource="&java;JavaAPIPart"/>
		<rdfs:seeAlso rdf:resource="&android-2_3;JavaSecurity"/>
		<rdfs:seeAlso rdf:resource="&android-2_3;JavaUtil"/>
		<rdfs:seeAlso rdf:resource="&android-2_3;JavaLang"/>
		<rdfs:comment xml:lang="en">Java API part implementing the java.security.acl package for Android 2.3</rdfs:comment>
	</owl:Class>
	<owl:Class rdf:about="&android-2_3;JavaSql">
		<owl:equivalentClass rdf:resource="&java-se-6;JavaSql"/>
		<rdfs:subClassOf rdf:resource="&android-2_2;JavaSql"/>
		<rdfs:seeAlso rdf:resource="&android-2_3;JavaSecurity"/>
		<rdfs:seeAlso rdf:resource="&android-2_3;JavaIo"/>
		<rdfs:seeAlso rdf:resource="&android-2_3;JavaLang"/>
		<rdfs:seeAlso rdf:resource="&android-2_3;JavaNet"/>
		<rdfs:seeAlso rdf:resource="&android-2_3;JavaUtil"/>
		<rdfs:seeAlso rdf:resource="&android-2_3;JavaxXmlTransform"/>
		<rdfs:seeAlso rdf:resource="&android-2_3;JavaMath"/>
		<rdfs:comment xml:lang="en">Java API part implementing the java.sql package for Android 2.3</rdfs:comment>
	</owl:Class>
	<owl:Class rdf:about="&android-2_3;JavaNio">
		<owl:equivalentClass rdf:resource="&java-se-6;JavaNio"/>
		<rdfs:subClassOf rdf:resource="&android-2_2;JavaNio"/>
		<rdfs:seeAlso rdf:resource="&android-2_3;JavaLang"/>
		<rdfs:comment xml:lang="en">Java API part implementing the java.nio package for Android 2.3</rdfs:comment>
	</owl:Class>
	<owl:Class rdf:about="&android-2_3;JavaNioChannels">
		<owl:equivalentClass rdf:resource="&java-se-6;JavaNioChannels"/>
		<owl:equivalentClass rdf:resource="&android-2_2;JavaNioChannels"/>
		<rdfs:subClassOf rdf:resource="&java;JavaAPIPart"/>
		<rdfs:seeAlso rdf:resource="&android-2_3;JavaNioChannelsSpi"/>
		<rdfs:seeAlso rdf:resource="&android-2_3;JavaNioCharset"/>
		<rdfs:seeAlso rdf:resource="&android-2_3;JavaIo"/>
		<rdfs:seeAlso rdf:resource="&android-2_3;JavaLang"/>
		<rdfs:seeAlso rdf:resource="&android-2_3;JavaNio"/>
		<rdfs:seeAlso rdf:resource="&android-2_3;JavaNet"/>
		<rdfs:seeAlso rdf:resource="&android-2_3;JavaUtil"/>
		<rdfs:comment xml:lang="en">Java API part implementing the java.nio.channels package for Android 2.3</rdfs:comment>
	</owl:Class>
	<owl:Class rdf:about="&android-2_3;JavaNioChannelsSpi">
		<owl:equivalentClass rdf:resource="&java-se-6;JavaNioChannelsSpi"/>
		<owl:equivalentClass rdf:resource="&android-2_2;JavaNioChannelsSpi"/>
		<rdfs:subClassOf rdf:resource="&java;JavaAPIPart"/>
		<rdfs:seeAlso rdf:resource="&android-2_3;JavaNioChannels"/>
		<rdfs:seeAlso rdf:resource="&android-2_3;JavaUtil"/>
		<rdfs:seeAlso rdf:resource="&android-2_3;JavaLang"/>
		<rdfs:comment xml:lang="en">Java API part implementing the java.nio.channels.spi package for Android 2.3</rdfs:comment>
	</owl:Class>
	<owl:Class rdf:about="&android-2_3;JavaNioCharset">
		<owl:equivalentClass rdf:resource="&java-se-6;JavaNioCharset"/>
		<owl:equivalentClass rdf:resource="&android-2_2;JavaNioCharset"/>
		<rdfs:subClassOf rdf:resource="&java;JavaAPIPart"/>
		<rdfs:seeAlso rdf:resource="&android-2_3;JavaIo"/>
		<rdfs:seeAlso rdf:resource="&android-2_3;JavaLang"/>
		<rdfs:seeAlso rdf:resource="&android-2_3;JavaNio"/>
		<rdfs:seeAlso rdf:resource="&android-2_3;JavaUtil"/>
		<rdfs:comment xml:lang="en">Java API part implementing the java.nio.charset package for Android 2.3</rdfs:comment>
	</owl:Class>
	<owl:Class rdf:about="&android-2_3;JavaNioCharsetSpi">
		<owl:equivalentClass rdf:resource="&java-se-6;JavaNioCharsetSpi"/>
		<owl:equivalentClass rdf:resource="&android-2_2;JavaNioCharsetSpi"/>
		<rdfs:subClassOf rdf:resource="&java;JavaAPIPart"/>
		<rdfs:seeAlso rdf:resource="&android-2_3;JavaUtil"/>
		<rdfs:seeAlso rdf:resource="&android-2_3;JavaNioCharset"/>
		<rdfs:seeAlso rdf:resource="&android-2_3;JavaLang"/>
		<rdfs:comment xml:lang="en">Java API part implementing the java.nio.charset.spi package for Android 2.3</rdfs:comment>
	</owl:Class>
	<owl:Class rdf:about="&android-2_3;JavaBeans">
		<owl:equivalentClass rdf:resource="&android-2_2;JavaBeans"/>
		<rdfs:subClassOf rdf:resource="&java;JavaAPIPart"/>
		<rdfs:seeAlso rdf:resource="&android-2_3;JavaUtil"/>
		<rdfs:seeAlso rdf:resource="&android-2_3;JavaIo"/>
		<rdfs:seeAlso rdf:resource="&android-2_3;JavaLang"/>
		<rdfs:comment xml:lang="en">Java API part implementing the java.beans package for Android 2.3</rdfs:comment>
	</owl:Class>
	<owl:Class rdf:about="&android-2_3;JavaText">
		<rdfs:subClassOf rdf:resource="&java-se-6;JavaText"/>
		<rdfs:seeAlso rdf:resource="&android-2_3;JavaIo"/>
		<rdfs:seeAlso rdf:resource="&android-2_3;JavaLang"/>
		<rdfs:seeAlso rdf:resource="&android-2_3;JavaUtil"/>
		<rdfs:seeAlso rdf:resource="&android-2_3;JavaMath"/>
		<rdfs:comment xml:lang="en">Java API part implementing the java.text package for Android 2.3</rdfs:comment>
	</owl:Class>
	<owl:Class rdf:about="&android-2_3;JavaAwtFont">
		<rdfs:subClassOf rdf:resource="&android-2_2;JavaAwtFont"/>
		<rdfs:seeAlso rdf:resource="&android-2_3;JavaText"/>
		<rdfs:seeAlso rdf:resource="&android-2_3;JavaIo"/>
		<rdfs:seeAlso rdf:resource="&android-2_3;JavaLang"/>
		<rdfs:comment xml:lang="en">Java API part implementing the java.awt.font package for Android 2.3</rdfs:comment>
	</owl:Class>
	<owl:Class rdf:about="&android-2_3;OrgXmlSax">
		<owl:equivalentClass rdf:resource="&java-se-6;OrgXmlSax"/>
		<owl:equivalentClass rdf:resource="&android-2_2;OrgXmlSax"/>
		<rdfs:subClassOf rdf:resource="&java;JavaAPIPart"/>
		<rdfs:seeAlso rdf:resource="&android-2_3;JavaUtil"/>
		<rdfs:seeAlso rdf:resource="&android-2_3;JavaIo"/>
		<rdfs:seeAlso rdf:resource="&android-2_3;JavaLang"/>
		<rdfs:comment xml:lang="en">Java API part implementing the org.xml.sax package for Android 2.3</rdfs:comment>
	</owl:Class>
	<owl:Class rdf:about="&android-2_3;OrgXmlSaxExt">
		<owl:equivalentClass rdf:resource="&java-se-6;OrgXmlSaxExt"/>
		<owl:equivalentClass rdf:resource="&android-2_2;OrgXmlSaxExt"/>
		<rdfs:subClassOf rdf:resource="&java;JavaAPIPart"/>
		<rdfs:seeAlso rdf:resource="&android-2_3;OrgXmlSax"/>
		<rdfs:seeAlso rdf:resource="&android-2_3;OrgXmlSaxHelpers"/>
		<rdfs:seeAlso rdf:resource="&android-2_3;JavaLang"/>
		<rdfs:comment xml:lang="en">Java API part implementing the org.xml.sax.ext package for Android 2.3</rdfs:comment>
	</owl:Class>
	<owl:Class rdf:about="&android-2_3;OrgXmlSaxHelpers">
		<owl:equivalentClass rdf:resource="&java-se-6;OrgXmlSaxHelpers"/>
		<owl:equivalentClass rdf:resource="&android-2_2;OrgXmlSaxHelpers"/>
		<rdfs:subClassOf rdf:resource="&java;JavaAPIPart"/>
		<rdfs:seeAlso rdf:resource="&android-2_3;OrgXmlSax"/>
		<rdfs:seeAlso rdf:resource="&android-2_3;JavaLang"/>
		<rdfs:seeAlso rdf:resource="&android-2_3;JavaUtil"/>
		<rdfs:comment xml:lang="en">Java API part implementing the org.xml.sax.helpers package for Android 2.3</rdfs:comment>
	</owl:Class>
	<owl:Class rdf:about="&android-2_3;OrgW3cDom">
		<owl:equivalentClass rdf:resource="&java-se-6;OrgW3cDom"/>
		<owl:equivalentClass rdf:resource="&android-2_2;OrgW3cDom"/>
		<rdfs:subClassOf rdf:resource="&java;JavaAPIPart"/>
		<rdfs:seeAlso rdf:resource="&android-2_3;JavaLang"/>
		<rdfs:comment xml:lang="en">Java API part implementing the org.w3c.dom package for Android 2.3</rdfs:comment>
	</owl:Class>
	<owl:Class rdf:about="&android-2_3;OrgW3cDomLs">
		<owl:equivalentClass rdf:resource="&android-2_2;OrgW3cDomLs"/>
		<rdfs:subClassOf rdf:resource="&java;JavaAPIPart"/>
		<rdfs:seeAlso rdf:resource="&android-2_3;JavaIo"/>
		<rdfs:seeAlso rdf:resource="&android-2_3;JavaLang"/>
		<rdfs:seeAlso rdf:resource="&android-2_3;OrgW3cDom"/>
		<rdfs:comment xml:lang="en">Java API part implementing the org.w3c.dom.ls package for Android 2.3</rdfs:comment>
	</owl:Class>
	<owl:Class rdf:about="&android-2_3;OrgXmlpullV1">
		<owl:equivalentClass rdf:resource="&android-2_2;OrgXmlpullV1"/>
		<rdfs:subClassOf rdf:resource="&java;JavaAPIPart"/>
		<rdfs:seeAlso rdf:resource="&android-2_3;JavaIo"/>
		<rdfs:seeAlso rdf:resource="&android-2_3;JavaLang"/>
		<rdfs:seeAlso rdf:resource="&android-2_3;JavaUtil"/>
		<rdfs:comment xml:lang="en">Java API part implementing the org.xmlpull.v1 package for Android 2.3</rdfs:comment>
	</owl:Class>
	<owl:Class rdf:about="&android-2_3;OrgXmlpullV1Sax2">
		<owl:equivalentClass rdf:resource="&android-2_2;OrgXmlpullV1Sax2"/>
		<rdfs:subClassOf rdf:resource="&java;JavaAPIPart"/>
		<rdfs:seeAlso rdf:resource="&android-2_3;OrgXmlSax"/>
		<rdfs:seeAlso rdf:resource="&android-2_3;OrgXmlpullV1"/>
		<rdfs:seeAlso rdf:resource="&android-2_3;JavaLang"/>
		<rdfs:comment xml:lang="en">Java API part implementing the org.xmlpull.v1.sax2 package for Android 2.3</rdfs:comment>
	</owl:Class>
	<owl:Class rdf:about="&android-2_3;OrgApacheHttp">
		<owl:equivalentClass rdf:resource="&android-2_2;OrgApacheHttp"/>
		<rdfs:subClassOf rdf:resource="&java;JavaAPIPart"/>
		<rdfs:seeAlso rdf:resource="&android-2_3;JavaIo"/>
		<rdfs:seeAlso rdf:resource="&android-2_3;JavaLang"/>
		<rdfs:seeAlso rdf:resource="&android-2_3;OrgApacheHttpProtocol"/>
		<rdfs:seeAlso rdf:resource="&android-2_3;OrgApacheHttpParams"/>
		<rdfs:seeAlso rdf:resource="&android-2_3;JavaNet"/>
		<rdfs:seeAlso rdf:resource="&android-2_3;OrgApacheHttpUtil"/>
		<rdfs:seeAlso rdf:resource="&android-2_3;JavaUtil"/>
		<rdfs:comment xml:lang="en">Java API part implementing the org.apache.http package for Android 2.3</rdfs:comment>
	</owl:Class>
	<owl:Class rdf:about="&android-2_3;OrgApacheHttpClient">
		<owl:equivalentClass rdf:resource="&android-2_2;OrgApacheHttpClient"/>
		<rdfs:subClassOf rdf:resource="&java;JavaAPIPart"/>
		<rdfs:seeAlso rdf:resource="&android-2_3;OrgApacheHttpCookie"/>
		<rdfs:seeAlso rdf:resource="&android-2_3;OrgApacheHttpConn"/>
		<rdfs:seeAlso rdf:resource="&android-2_3;JavaIo"/>
		<rdfs:seeAlso rdf:resource="&android-2_3;OrgApacheHttpAuth"/>
		<rdfs:seeAlso rdf:resource="&android-2_3;JavaLang"/>
		<rdfs:seeAlso rdf:resource="&android-2_3;OrgApacheHttpProtocol"/>
		<rdfs:seeAlso rdf:resource="&android-2_3;OrgApacheHttpClientMethods"/>
		<rdfs:seeAlso rdf:resource="&android-2_3;OrgApacheHttpParams"/>
		<rdfs:seeAlso rdf:resource="&android-2_3;JavaNet"/>
		<rdfs:seeAlso rdf:resource="&android-2_3;JavaUtil"/>
		<rdfs:seeAlso rdf:resource="&android-2_3;OrgApacheHttp"/>
		<rdfs:comment xml:lang="en">Java API part implementing the org.apache.http.client package for Android 2.3</rdfs:comment>
	</owl:Class>
	<owl:Class rdf:about="&android-2_3;OrgApacheHttpClientMethods">
		<owl:equivalentClass rdf:resource="&android-2_2;OrgApacheHttpClientMethods"/>
		<rdfs:subClassOf rdf:resource="&java;JavaAPIPart"/>
		<rdfs:seeAlso rdf:resource="&android-2_3;OrgApacheHttpConn"/>
		<rdfs:seeAlso rdf:resource="&android-2_3;JavaLang"/>
		<rdfs:seeAlso rdf:resource="&android-2_3;OrgApacheHttpMessage"/>
		<rdfs:seeAlso rdf:resource="&android-2_3;JavaNet"/>
		<rdfs:seeAlso rdf:resource="&android-2_3;JavaUtil"/>
		<rdfs:seeAlso rdf:resource="&android-2_3;OrgApacheHttp"/>
		<rdfs:comment xml:lang="en">Java API part implementing the org.apache.http.client.methods package for Android 2.3</rdfs:comment>
	</owl:Class>
	<owl:Class rdf:about="&android-2_3;OrgApacheHttpClientEntity">
		<owl:equivalentClass rdf:resource="&android-2_2;OrgApacheHttpClientEntity"/>
		<rdfs:subClassOf rdf:resource="&java;JavaAPIPart"/>
		<rdfs:seeAlso rdf:resource="&android-2_3;JavaUtil"/>
		<rdfs:seeAlso rdf:resource="&android-2_3;OrgApacheHttpEntity"/>
		<rdfs:seeAlso rdf:resource="&android-2_3;JavaLang"/>
		<rdfs:comment xml:lang="en">Java API part implementing the org.apache.http.client.entity package for Android 2.3</rdfs:comment>
	</owl:Class>
	<owl:Class rdf:about="&android-2_3;OrgApacheHttpClientParams">
		<owl:equivalentClass rdf:resource="&android-2_2;OrgApacheHttpClientParams"/>
		<rdfs:subClassOf rdf:resource="&java;JavaAPIPart"/>
		<rdfs:seeAlso rdf:resource="&android-2_3;OrgApacheHttpConn"/>
		<rdfs:seeAlso rdf:resource="&android-2_3;OrgApacheHttpConnParams"/>
		<rdfs:seeAlso rdf:resource="&android-2_3;JavaLang"/>
		<rdfs:seeAlso rdf:resource="&android-2_3;OrgApacheHttpCookieParams"/>
		<rdfs:seeAlso rdf:resource="&android-2_3;OrgApacheHttpAuthParams"/>
		<rdfs:seeAlso rdf:resource="&android-2_3;OrgApacheHttpParams"/>
		<rdfs:seeAlso rdf:resource="&android-2_3;JavaUtil"/>
		<rdfs:seeAlso rdf:resource="&android-2_3;OrgApacheHttp"/>
		<rdfs:comment xml:lang="en">Java API part implementing the org.apache.http.client.params package for Android 2.3</rdfs:comment>
	</owl:Class>
	<owl:Class rdf:about="&android-2_3;OrgApacheHttpClientProtocol">
		<owl:equivalentClass rdf:resource="&android-2_2;OrgApacheHttpClientProtocol"/>
		<rdfs:subClassOf rdf:resource="&java;JavaAPIPart"/>
		<rdfs:seeAlso rdf:resource="&android-2_3;OrgApacheHttpCookie"/>
		<rdfs:seeAlso rdf:resource="&android-2_3;OrgApacheHttpAuth"/>
		<rdfs:seeAlso rdf:resource="&android-2_3;JavaLang"/>
		<rdfs:seeAlso rdf:resource="&android-2_3;OrgApacheHttpProtocol"/>
		<rdfs:seeAlso rdf:resource="&android-2_3;JavaUtil"/>
		<rdfs:seeAlso rdf:resource="&android-2_3;OrgApacheHttp"/>
		<rdfs:seeAlso rdf:resource="&android-2_3;OrgApacheHttpClient"/>
		<rdfs:comment xml:lang="en">Java API part implementing the org.apache.http.client.protocol package for Android 2.3</rdfs:comment>
	</owl:Class>
	<owl:Class rdf:about="&android-2_3;OrgApacheHttpClientUtils">
		<owl:equivalentClass rdf:resource="&android-2_2;OrgApacheHttpClientUtils"/>
		<rdfs:subClassOf rdf:resource="&java;JavaAPIPart"/>
		<rdfs:seeAlso rdf:resource="&android-2_3;JavaNet"/>
		<rdfs:seeAlso rdf:resource="&android-2_3;JavaUtil"/>
		<rdfs:seeAlso rdf:resource="&android-2_3;OrgApacheHttp"/>
		<rdfs:seeAlso rdf:resource="&android-2_3;JavaLang"/>
		<rdfs:comment xml:lang="en">Java API part implementing the org.apache.http.client.utils package for Android 2.3</rdfs:comment>
	</owl:Class>
	<owl:Class rdf:about="&android-2_3;OrgApacheHttpParams">
		<owl:equivalentClass rdf:resource="&android-2_2;OrgApacheHttpParams"/>
		<rdfs:subClassOf rdf:resource="&java;JavaAPIPart"/>
		<rdfs:seeAlso rdf:resource="&android-2_3;JavaIo"/>
		<rdfs:seeAlso rdf:resource="&android-2_3;OrgApacheHttp"/>
		<rdfs:seeAlso rdf:resource="&android-2_3;JavaLang"/>
		<rdfs:comment xml:lang="en">Java API part implementing the org.apache.http.params package for Android 2.3</rdfs:comment>
	</owl:Class>
	<owl:Class rdf:about="&android-2_3;OrgApacheHttpConn">
		<owl:equivalentClass rdf:resource="&android-2_2;OrgApacheHttpConn"/>
		<rdfs:subClassOf rdf:resource="&java;JavaAPIPart"/>
		<rdfs:seeAlso rdf:resource="&android-2_3;JavaUtilConcurrent"/>
		<rdfs:seeAlso rdf:resource="&android-2_3;JavaxNetSsl"/>
		<rdfs:seeAlso rdf:resource="&android-2_3;OrgApacheHttpEntity"/>
		<rdfs:seeAlso rdf:resource="&android-2_3;JavaIo"/>
		<rdfs:seeAlso rdf:resource="&android-2_3;JavaLang"/>
		<rdfs:seeAlso rdf:resource="&android-2_3;OrgApacheHttpProtocol"/>
		<rdfs:seeAlso rdf:resource="&android-2_3;OrgApacheHttpParams"/>
		<rdfs:seeAlso rdf:resource="&android-2_3;JavaNet"/>
		<rdfs:seeAlso rdf:resource="&android-2_3;OrgApacheHttpConnRouting"/>
		<rdfs:seeAlso rdf:resource="&android-2_3;OrgApacheHttp"/>
		<rdfs:seeAlso rdf:resource="&android-2_3;OrgApacheHttpConnScheme"/>
		<rdfs:comment xml:lang="en">Java API part implementing the org.apache.http.conn package for Android 2.3</rdfs:comment>
	</owl:Class>
	<owl:Class rdf:about="&android-2_3;OrgApacheHttpConnSsl">
		<owl:equivalentClass rdf:resource="&android-2_2;OrgApacheHttpConnSsl"/>
		<rdfs:subClassOf rdf:resource="&java;JavaAPIPart"/>
		<rdfs:seeAlso rdf:resource="&android-2_3;JavaSecurity"/>
		<rdfs:seeAlso rdf:resource="&android-2_3;JavaxNetSsl"/>
		<rdfs:seeAlso rdf:resource="&android-2_3;JavaLang"/>
		<rdfs:seeAlso rdf:resource="&android-2_3;JavaSecurityCert"/>
		<rdfs:seeAlso rdf:resource="&android-2_3;OrgApacheHttpParams"/>
		<rdfs:seeAlso rdf:resource="&android-2_3;JavaNet"/>
		<rdfs:seeAlso rdf:resource="&android-2_3;OrgApacheHttpConnScheme"/>
		<rdfs:comment xml:lang="en">Java API part implementing the org.apache.http.conn.ssl package for Android 2.3</rdfs:comment>
	</owl:Class>
	<owl:Class rdf:about="&android-2_3;OrgApacheHttpConnRouting">
		<rdfs:subClassOf rdf:resource="&android-2_2;OrgApacheHttpConnRouting"/>
		<rdfs:seeAlso rdf:resource="&android-2_3;JavaNet"/>
		<rdfs:seeAlso rdf:resource="&android-2_3;OrgApacheHttp"/>
		<rdfs:seeAlso rdf:resource="&android-2_3;JavaLang"/>
		<rdfs:seeAlso rdf:resource="&android-2_3;OrgApacheHttpProtocol"/>
		<rdfs:comment xml:lang="en">Java API part implementing the org.apache.http.conn.routing package for Android 2.3</rdfs:comment>
	</owl:Class>
	<owl:Class rdf:about="&android-2_3;OrgApacheHttpConnScheme">
		<owl:equivalentClass rdf:resource="&android-2_2;OrgApacheHttpConnScheme"/>
		<rdfs:subClassOf rdf:resource="&java;JavaAPIPart"/>
		<rdfs:seeAlso rdf:resource="&android-2_3;JavaNet"/>
		<rdfs:seeAlso rdf:resource="&android-2_3;JavaUtil"/>
		<rdfs:seeAlso rdf:resource="&android-2_3;OrgApacheHttp"/>
		<rdfs:seeAlso rdf:resource="&android-2_3;JavaLang"/>
		<rdfs:seeAlso rdf:resource="&android-2_3;OrgApacheHttpParams"/>
		<rdfs:comment xml:lang="en">Java API part implementing the org.apache.http.conn.scheme package for Android 2.3</rdfs:comment>
	</owl:Class>
	<owl:Class rdf:about="&android-2_3;OrgApacheHttpConnUtil">
		<owl:equivalentClass rdf:resource="&android-2_2;OrgApacheHttpConnUtil"/>
		<rdfs:subClassOf rdf:resource="&java;JavaAPIPart"/>
		<rdfs:seeAlso rdf:resource="&android-2_3;JavaLang"/>
		<rdfs:comment xml:lang="en">Java API part implementing the org.apache.http.conn.util package for Android 2.3</rdfs:comment>
	</owl:Class>
	<owl:Class rdf:about="&android-2_3;OrgApacheHttpConnParams">
		<owl:equivalentClass rdf:resource="&android-2_2;OrgApacheHttpConnParams"/>
		<rdfs:subClassOf rdf:resource="&java;JavaAPIPart"/>
		<rdfs:seeAlso rdf:resource="&android-2_3;JavaNet"/>
		<rdfs:seeAlso rdf:resource="&android-2_3;OrgApacheHttpConnRouting"/>
		<rdfs:seeAlso rdf:resource="&android-2_3;JavaUtil"/>
		<rdfs:seeAlso rdf:resource="&android-2_3;OrgApacheHttp"/>
		<rdfs:seeAlso rdf:resource="&android-2_3;JavaLang"/>
		<rdfs:seeAlso rdf:resource="&android-2_3;OrgApacheHttpParams"/>
		<rdfs:comment xml:lang="en">Java API part implementing the org.apache.http.conn.params package for Android 2.3</rdfs:comment>
	</owl:Class>
	<owl:Class rdf:about="&android-2_3;OrgApacheHttpProtocol">
		<owl:equivalentClass rdf:resource="&android-2_2;OrgApacheHttpProtocol"/>
		<rdfs:subClassOf rdf:resource="&java;JavaAPIPart"/>
		<rdfs:seeAlso rdf:resource="&android-2_3;JavaLang"/>
		<rdfs:seeAlso rdf:resource="&android-2_3;OrgApacheHttpParams"/>
		<rdfs:seeAlso rdf:resource="&android-2_3;JavaUtil"/>
		<rdfs:seeAlso rdf:resource="&android-2_3;OrgApacheHttp"/>
		<rdfs:comment xml:lang="en">Java API part implementing the org.apache.http.protocol package for Android 2.3</rdfs:comment>
	</owl:Class>
	<owl:Class rdf:about="&android-2_3;OrgApacheHttpEntity">
		<owl:equivalentClass rdf:resource="&android-2_2;OrgApacheHttpEntity"/>
		<rdfs:subClassOf rdf:resource="&java;JavaAPIPart"/>
		<rdfs:seeAlso rdf:resource="&android-2_3;JavaIo"/>
		<rdfs:seeAlso rdf:resource="&android-2_3;OrgApacheHttp"/>
		<rdfs:seeAlso rdf:resource="&android-2_3;JavaLang"/>
		<rdfs:comment xml:lang="en">Java API part implementing the org.apache.http.entity package for Android 2.3</rdfs:comment>
	</owl:Class>
	<owl:Class rdf:about="&android-2_3;OrgApacheHttpImpl">
		<owl:equivalentClass rdf:resource="&android-2_2;OrgApacheHttpImpl"/>
		<rdfs:subClassOf rdf:resource="&java;JavaAPIPart"/>
		<rdfs:seeAlso rdf:resource="&android-2_3;OrgApacheHttpImplEntity"/>
		<rdfs:seeAlso rdf:resource="&android-2_3;OrgApacheHttpIo"/>
		<rdfs:seeAlso rdf:resource="&android-2_3;JavaLang"/>
		<rdfs:seeAlso rdf:resource="&android-2_3;OrgApacheHttpProtocol"/>
		<rdfs:seeAlso rdf:resource="&android-2_3;OrgApacheHttpParams"/>
		<rdfs:seeAlso rdf:resource="&android-2_3;JavaNet"/>
		<rdfs:seeAlso rdf:resource="&android-2_3;JavaUtil"/>
		<rdfs:seeAlso rdf:resource="&android-2_3;OrgApacheHttp"/>
		<rdfs:comment xml:lang="en">Java API part implementing the org.apache.http.impl package for Android 2.3</rdfs:comment>
	</owl:Class>
	<owl:Class rdf:about="&android-2_3;OrgApacheHttpImplEntity">
		<owl:equivalentClass rdf:resource="&android-2_2;OrgApacheHttpImplEntity"/>
		<rdfs:subClassOf rdf:resource="&java;JavaAPIPart"/>
		<rdfs:seeAlso rdf:resource="&android-2_3;OrgApacheHttpIo"/>
		<rdfs:seeAlso rdf:resource="&android-2_3;JavaIo"/>
		<rdfs:seeAlso rdf:resource="&android-2_3;OrgApacheHttp"/>
		<rdfs:seeAlso rdf:resource="&android-2_3;OrgApacheHttpEntity"/>
		<rdfs:seeAlso rdf:resource="&android-2_3;JavaLang"/>
		<rdfs:comment xml:lang="en">Java API part implementing the org.apache.http.impl.entity package for Android 2.3</rdfs:comment>
	</owl:Class>
	<owl:Class rdf:about="&android-2_3;OrgApacheHttpImplConn">
		<owl:equivalentClass rdf:resource="&android-2_2;OrgApacheHttpImplConn"/>
		<rdfs:subClassOf rdf:resource="&java;JavaAPIPart"/>
		<rdfs:seeAlso rdf:resource="&android-2_3;OrgApacheHttpConn"/>
		<rdfs:seeAlso rdf:resource="&android-2_3;OrgApacheHttpImpl"/>
		<rdfs:seeAlso rdf:resource="&android-2_3;OrgApacheHttpMessage"/>
		<rdfs:seeAlso rdf:resource="&android-2_3;OrgApacheHttpImplIo"/>
		<rdfs:seeAlso rdf:resource="&android-2_3;OrgApacheHttpUtil"/>
		<rdfs:seeAlso rdf:resource="&android-2_3;OrgApacheCommonsLogging"/>
		<rdfs:seeAlso rdf:resource="&android-2_3;OrgApacheHttpConnRouting"/>
		<rdfs:seeAlso rdf:resource="&android-2_3;OrgApacheHttpConnScheme"/>
		<rdfs:seeAlso rdf:resource="&android-2_3;JavaUtilConcurrent"/>
		<rdfs:seeAlso rdf:resource="&android-2_3;JavaxNetSsl"/>
		<rdfs:seeAlso rdf:resource="&android-2_3;OrgApacheHttpIo"/>
		<rdfs:seeAlso rdf:resource="&android-2_3;JavaIo"/>
		<rdfs:seeAlso rdf:resource="&android-2_3;JavaLang"/>
		<rdfs:seeAlso rdf:resource="&android-2_3;OrgApacheHttpProtocol"/>
		<rdfs:seeAlso rdf:resource="&android-2_3;OrgApacheHttpParams"/>
		<rdfs:seeAlso rdf:resource="&android-2_3;JavaNet"/>
		<rdfs:seeAlso rdf:resource="&android-2_3;JavaUtil"/>
		<rdfs:seeAlso rdf:resource="&android-2_3;OrgApacheHttp"/>
		<rdfs:comment xml:lang="en">Java API part implementing the org.apache.http.impl.conn package for Android 2.3</rdfs:comment>
	</owl:Class>
	<owl:Class rdf:about="&android-2_3;OrgApacheHttpImplConnTsccm">
		<owl:equivalentClass rdf:resource="&android-2_2;OrgApacheHttpImplConnTsccm"/>
		<rdfs:subClassOf rdf:resource="&java;JavaAPIPart"/>
		<rdfs:seeAlso rdf:resource="&android-2_3;OrgApacheHttpConn"/>
		<rdfs:seeAlso rdf:resource="&android-2_3;JavaUtilConcurrentLocks"/>
		<rdfs:seeAlso rdf:resource="&android-2_3;OrgApacheHttpConnRouting"/>
		<rdfs:seeAlso rdf:resource="&android-2_3;OrgApacheHttpConnScheme"/>
		<rdfs:seeAlso rdf:resource="&android-2_3;JavaUtilConcurrent"/>
		<rdfs:seeAlso rdf:resource="&android-2_3;JavaLang"/>
		<rdfs:seeAlso rdf:resource="&android-2_3;OrgApacheHttpImplConn"/>
		<rdfs:seeAlso rdf:resource="&android-2_3;OrgApacheHttpParams"/>
		<rdfs:seeAlso rdf:resource="&android-2_3;JavaLangRef"/>
		<rdfs:seeAlso rdf:resource="&android-2_3;JavaUtil"/>
		<rdfs:comment xml:lang="en">Java API part implementing the org.apache.http.impl.conn.tsccm package for Android 2.3</rdfs:comment>
	</owl:Class>
	<owl:Class rdf:about="&android-2_3;OrgApacheHttpImplIo">
		<owl:equivalentClass rdf:resource="&android-2_2;OrgApacheHttpImplIo"/>
		<rdfs:subClassOf rdf:resource="&java;JavaAPIPart"/>
		<rdfs:seeAlso rdf:resource="&android-2_3;OrgApacheHttpIo"/>
		<rdfs:seeAlso rdf:resource="&android-2_3;JavaIo"/>
		<rdfs:seeAlso rdf:resource="&android-2_3;JavaLang"/>
		<rdfs:seeAlso rdf:resource="&android-2_3;OrgApacheHttpParams"/>
		<rdfs:seeAlso rdf:resource="&android-2_3;OrgApacheHttpMessage"/>
		<rdfs:seeAlso rdf:resource="&android-2_3;JavaNet"/>
		<rdfs:seeAlso rdf:resource="&android-2_3;OrgApacheHttpUtil"/>
		<rdfs:seeAlso rdf:resource="&android-2_3;OrgApacheHttp"/>
		<rdfs:comment xml:lang="en">Java API part implementing the org.apache.http.impl.io package for Android 2.3</rdfs:comment>
	</owl:Class>
	<owl:Class rdf:about="&android-2_3;OrgApacheHttpImplCookie">
		<owl:equivalentClass rdf:resource="&android-2_2;OrgApacheHttpImplCookie"/>
		<rdfs:subClassOf rdf:resource="&java;JavaAPIPart"/>
		<rdfs:seeAlso rdf:resource="&android-2_3;OrgApacheHttpCookie"/>
		<rdfs:seeAlso rdf:resource="&android-2_3;JavaLang"/>
		<rdfs:seeAlso rdf:resource="&android-2_3;OrgApacheHttpParams"/>
		<rdfs:seeAlso rdf:resource="&android-2_3;OrgApacheHttpMessage"/>
		<rdfs:seeAlso rdf:resource="&android-2_3;OrgApacheHttpUtil"/>
		<rdfs:seeAlso rdf:resource="&android-2_3;JavaUtil"/>
		<rdfs:seeAlso rdf:resource="&android-2_3;OrgApacheHttp"/>
		<rdfs:comment xml:lang="en">Java API part implementing the org.apache.http.impl.cookie package for Android 2.3</rdfs:comment>
	</owl:Class>
	<owl:Class rdf:about="&android-2_3;OrgApacheHttpImplAuth">
		<owl:equivalentClass rdf:resource="&android-2_2;OrgApacheHttpImplAuth"/>
		<rdfs:subClassOf rdf:resource="&java;JavaAPIPart"/>
		<rdfs:seeAlso rdf:resource="&android-2_3;OrgApacheHttpAuth"/>
		<rdfs:seeAlso rdf:resource="&android-2_3;JavaLang"/>
		<rdfs:seeAlso rdf:resource="&android-2_3;OrgApacheHttpParams"/>
		<rdfs:seeAlso rdf:resource="&android-2_3;OrgApacheHttpUtil"/>
		<rdfs:seeAlso rdf:resource="&android-2_3;JavaUtil"/>
		<rdfs:seeAlso rdf:resource="&android-2_3;OrgApacheHttp"/>
		<rdfs:comment xml:lang="en">Java API part implementing the org.apache.http.impl.auth package for Android 2.3</rdfs:comment>
	</owl:Class>
	<owl:Class rdf:about="&android-2_3;OrgApacheHttpImplClient">
		<owl:equivalentClass rdf:resource="&android-2_2;OrgApacheHttpImplClient"/>
		<rdfs:subClassOf rdf:resource="&java;JavaAPIPart"/>
		<rdfs:seeAlso rdf:resource="&android-2_3;OrgApacheHttpCookie"/>
		<rdfs:seeAlso rdf:resource="&android-2_3;OrgApacheHttpConn"/>
		<rdfs:seeAlso rdf:resource="&android-2_3;OrgApacheHttpClientMethods"/>
		<rdfs:seeAlso rdf:resource="&android-2_3;OrgApacheHttpMessage"/>
		<rdfs:seeAlso rdf:resource="&android-2_3;OrgApacheHttpConnRouting"/>
		<rdfs:seeAlso rdf:resource="&android-2_3;JavaIo"/>
		<rdfs:seeAlso rdf:resource="&android-2_3;OrgApacheHttpAuth"/>
		<rdfs:seeAlso rdf:resource="&android-2_3;JavaLang"/>
		<rdfs:seeAlso rdf:resource="&android-2_3;OrgApacheHttpProtocol"/>
		<rdfs:seeAlso rdf:resource="&android-2_3;OrgApacheHttpParams"/>
		<rdfs:seeAlso rdf:resource="&android-2_3;JavaNet"/>
		<rdfs:seeAlso rdf:resource="&android-2_3;JavaUtil"/>
		<rdfs:seeAlso rdf:resource="&android-2_3;OrgApacheHttp"/>
		<rdfs:seeAlso rdf:resource="&android-2_3;OrgApacheHttpClient"/>
		<rdfs:comment xml:lang="en">Java API part implementing the org.apache.http.impl.client package for Android 2.3</rdfs:comment>
	</owl:Class>
	<owl:Class rdf:about="&android-2_3;OrgApacheHttpIo">
		<owl:equivalentClass rdf:resource="&android-2_2;OrgApacheHttpIo"/>
		<rdfs:subClassOf rdf:resource="&java;JavaAPIPart"/>
		<rdfs:seeAlso rdf:resource="&android-2_3;OrgApacheHttpUtil"/>
		<rdfs:seeAlso rdf:resource="&android-2_3;OrgApacheHttp"/>
		<rdfs:seeAlso rdf:resource="&android-2_3;JavaLang"/>
		<rdfs:comment xml:lang="en">Java API part implementing the org.apache.http.io package for Android 2.3</rdfs:comment>
	</owl:Class>
	<owl:Class rdf:about="&android-2_3;OrgApacheHttpUtil">
		<owl:equivalentClass rdf:resource="&android-2_2;OrgApacheHttpUtil"/>
		<rdfs:subClassOf rdf:resource="&java;JavaAPIPart"/>
		<rdfs:seeAlso rdf:resource="&android-2_3;JavaUtil"/>
		<rdfs:seeAlso rdf:resource="&android-2_3;OrgApacheHttp"/>
		<rdfs:seeAlso rdf:resource="&android-2_3;JavaLang"/>
		<rdfs:comment xml:lang="en">Java API part implementing the org.apache.http.util package for Android 2.3</rdfs:comment>
	</owl:Class>
	<owl:Class rdf:about="&android-2_3;OrgApacheHttpMessage">
		<owl:equivalentClass rdf:resource="&android-2_2;OrgApacheHttpMessage"/>
		<rdfs:subClassOf rdf:resource="&java;JavaAPIPart"/>
		<rdfs:seeAlso rdf:resource="&android-2_3;JavaLang"/>
		<rdfs:seeAlso rdf:resource="&android-2_3;OrgApacheHttpParams"/>
		<rdfs:seeAlso rdf:resource="&android-2_3;OrgApacheHttpUtil"/>
		<rdfs:seeAlso rdf:resource="&android-2_3;JavaUtil"/>
		<rdfs:seeAlso rdf:resource="&android-2_3;OrgApacheHttp"/>
		<rdfs:comment xml:lang="en">Java API part implementing the org.apache.http.message package for Android 2.3</rdfs:comment>
	</owl:Class>
	<owl:Class rdf:about="&android-2_3;OrgApacheHttpCookie">
		<owl:equivalentClass rdf:resource="&android-2_2;OrgApacheHttpCookie"/>
		<rdfs:subClassOf rdf:resource="&java;JavaAPIPart"/>
		<rdfs:seeAlso rdf:resource="&android-2_3;JavaUtil"/>
		<rdfs:seeAlso rdf:resource="&android-2_3;JavaIo"/>
		<rdfs:seeAlso rdf:resource="&android-2_3;OrgApacheHttp"/>
		<rdfs:seeAlso rdf:resource="&android-2_3;JavaLang"/>
		<rdfs:seeAlso rdf:resource="&android-2_3;OrgApacheHttpParams"/>
		<rdfs:comment xml:lang="en">Java API part implementing the org.apache.http.cookie package for Android 2.3</rdfs:comment>
	</owl:Class>
	<owl:Class rdf:about="&android-2_3;OrgApacheHttpCookieParams">
		<owl:equivalentClass rdf:resource="&android-2_2;OrgApacheHttpCookieParams"/>
		<rdfs:subClassOf rdf:resource="&java;JavaAPIPart"/>
		<rdfs:seeAlso rdf:resource="&android-2_3;JavaUtil"/>
		<rdfs:seeAlso rdf:resource="&android-2_3;JavaLang"/>
		<rdfs:seeAlso rdf:resource="&android-2_3;OrgApacheHttpParams"/>
		<rdfs:comment xml:lang="en">Java API part implementing the org.apache.http.cookie.params package for Android 2.3</rdfs:comment>
	</owl:Class>
	<owl:Class rdf:about="&android-2_3;OrgApacheHttpAuth">
		<owl:equivalentClass rdf:resource="&android-2_2;OrgApacheHttpAuth"/>
		<rdfs:subClassOf rdf:resource="&java;JavaAPIPart"/>
		<rdfs:seeAlso rdf:resource="&android-2_3;JavaSecurity"/>
		<rdfs:seeAlso rdf:resource="&android-2_3;JavaUtil"/>
		<rdfs:seeAlso rdf:resource="&android-2_3;OrgApacheHttp"/>
		<rdfs:seeAlso rdf:resource="&android-2_3;JavaLang"/>
		<rdfs:seeAlso rdf:resource="&android-2_3;OrgApacheHttpParams"/>
		<rdfs:comment xml:lang="en">Java API part implementing the org.apache.http.auth package for Android 2.3</rdfs:comment>
	</owl:Class>
	<owl:Class rdf:about="&android-2_3;OrgApacheHttpAuthParams">
		<owl:equivalentClass rdf:resource="&android-2_2;OrgApacheHttpAuthParams"/>
		<rdfs:subClassOf rdf:resource="&java;JavaAPIPart"/>
		<rdfs:seeAlso rdf:resource="&android-2_3;JavaLang"/>
		<rdfs:seeAlso rdf:resource="&android-2_3;OrgApacheHttpParams"/>
		<rdfs:comment xml:lang="en">Java API part implementing the org.apache.http.auth.params package for Android 2.3</rdfs:comment>
	</owl:Class>
	<owl:Class rdf:about="&android-2_3;OrgApacheCommonsLogging">
		<owl:equivalentClass rdf:resource="&android-2_2;OrgApacheCommonsLogging"/>
		<rdfs:subClassOf rdf:resource="&java;JavaAPIPart"/>
		<rdfs:seeAlso rdf:resource="&android-2_3;JavaLang"/>
		<rdfs:comment xml:lang="en">Java API part implementing the org.apache.commons.logging package for Android 2.3</rdfs:comment>
	</owl:Class>
	<owl:Class rdf:about="&android-2_3;OrgJson">
		<owl:equivalentClass rdf:resource="&android-2_2;OrgJson"/>
		<rdfs:subClassOf rdf:resource="&java;JavaAPIPart"/>
		<rdfs:seeAlso rdf:resource="&android-2_3;JavaUtil"/>
		<rdfs:seeAlso rdf:resource="&android-2_3;JavaLang"/>
		<rdfs:comment xml:lang="en">Java API part implementing the org.json package for Android 2.3</rdfs:comment>
	</owl:Class>
	<owl:Class rdf:about="&android-2_3;DalvikBytecode">
		<rdfs:subClassOf rdf:resource="&android-2_2;DalvikBytecode"/>
		<rdfs:comment xml:lang="en">Java API part implementing the dalvik.bytecode package for Android 2.3</rdfs:comment>
	</owl:Class>
	<owl:Class rdf:about="&android-2_3;DalvikAnnotation">
		<owl:equivalentClass rdf:resource="&android-2_2;DalvikAnnotation"/>
		<rdfs:subClassOf rdf:resource="&java;JavaAPIPart"/>
		<rdfs:seeAlso rdf:resource="&android-2_3;JavaLang"/>
		<rdfs:seeAlso rdf:resource="&android-2_3;JavaLangAnnotation"/>
		<rdfs:comment xml:lang="en">Java API part implementing the dalvik.annotation package for Android 2.3</rdfs:comment>
	</owl:Class>
	<owl:Class rdf:about="&android-2_3;DalvikSystem">
		<rdfs:subClassOf rdf:resource="&java;JavaAPIPart"/>
		<rdfs:seeAlso rdf:resource="&android-2_3;JavaNet"/>
		<rdfs:seeAlso rdf:resource="&android-2_3;JavaUtil"/>
		<rdfs:seeAlso rdf:resource="&android-2_3;JavaIo"/>
		<rdfs:seeAlso rdf:resource="&android-2_3;JavaLang"/>
		<rdfs:comment xml:lang="en">Java API part implementing the dalvik.system package for Android 2.3</rdfs:comment>
	</owl:Class>
	<owl:Class rdf:about="&android-2_3;JunitRunner">
		<owl:equivalentClass rdf:resource="&android-2_2;JunitRunner"/>
		<rdfs:subClassOf rdf:resource="&java;JavaAPIPart"/>
		<rdfs:seeAlso rdf:resource="&android-2_3;JunitFramework"/>
		<rdfs:seeAlso rdf:resource="&android-2_3;JavaUtil"/>
		<rdfs:seeAlso rdf:resource="&android-2_3;JavaLang"/>
		<rdfs:comment xml:lang="en">Java API part implementing the junit.runner package for Android 2.3</rdfs:comment>
	</owl:Class>
	<owl:Class rdf:about="&android-2_3;JunitFramework">
		<owl:equivalentClass rdf:resource="&android-2_2;JunitFramework"/>
		<rdfs:subClassOf rdf:resource="&java;JavaAPIPart"/>
		<rdfs:seeAlso rdf:resource="&android-2_3;JavaLangReflect"/>
		<rdfs:seeAlso rdf:resource="&android-2_3;JavaUtil"/>
		<rdfs:seeAlso rdf:resource="&android-2_3;JavaLang"/>
		<rdfs:comment xml:lang="en">Java API part implementing the junit.framework package for Android 2.3</rdfs:comment>
	</owl:Class>
	<owl:Class rdf:about="&android-2_3;Android">
		<rdfs:subClassOf rdf:resource="&java;JavaAPIPart"/>
		<rdfs:seeAlso rdf:resource="&android-2_3;JavaLang"/>
		<rdfs:comment xml:lang="en">Java API part implementing the android package for Android 2.3</rdfs:comment>
	</owl:Class>
	<owl:Class rdf:about="&android-2_3;AndroidContent">
		<rdfs:subClassOf rdf:resource="&android-2_2;AndroidContent"/>
		<rdfs:seeAlso rdf:resource="&android-2_3;AndroidView"/>
		<rdfs:seeAlso rdf:resource="&android-2_3;AndroidUtil"/>
		<rdfs:seeAlso rdf:resource="&android-2_3;AndroidNet"/>
		<rdfs:seeAlso rdf:resource="&android-2_3;OrgXmlpullV1"/>
		<rdfs:seeAlso rdf:resource="&android-2_3;AndroidDatabase"/>
		<rdfs:seeAlso rdf:resource="&android-2_3;AndroidAccounts"/>
		<rdfs:seeAlso rdf:resource="&android-2_3;AndroidContentRes"/>
		<rdfs:seeAlso rdf:resource="&android-2_3;AndroidOs"/>
		<rdfs:seeAlso rdf:resource="&android-2_3;AndroidContentPm"/>
		<rdfs:seeAlso rdf:resource="&android-2_3;AndroidGraphics"/>
		<rdfs:seeAlso rdf:resource="&android-2_3;JavaIo"/>
		<rdfs:seeAlso rdf:resource="&android-2_3;JavaLang"/>
		<rdfs:seeAlso rdf:resource="&android-2_3;AndroidDatabaseSqlite"/>
		<rdfs:seeAlso rdf:resource="&android-2_3;AndroidGraphicsDrawable"/>
		<rdfs:seeAlso rdf:resource="&android-2_3;JavaUtil"/>
		<rdfs:comment xml:lang="en">Java API part implementing the android.content package for Android 2.3</rdfs:comment>
	</owl:Class>
	<owl:Class rdf:about="&android-2_3;AndroidContentPm">
		<rdfs:subClassOf rdf:resource="&android-2_2;AndroidContentPm"/>
		<rdfs:seeAlso rdf:resource="&android-2_3;AndroidContent"/>
		<rdfs:seeAlso rdf:resource="&android-2_3;JavaLang"/>
		<rdfs:seeAlso rdf:resource="&android-2_3;AndroidGraphicsDrawable"/>
		<rdfs:seeAlso rdf:resource="&android-2_3;AndroidContentRes"/>
		<rdfs:seeAlso rdf:resource="&android-2_3;AndroidUtil"/>
		<rdfs:seeAlso rdf:resource="&android-2_3;AndroidOs"/>
		<rdfs:seeAlso rdf:resource="&android-2_3;JavaUtil"/>
		<rdfs:comment xml:lang="en">Java API part implementing the android.content.pm package for Android 2.3</rdfs:comment>
	</owl:Class>
	<owl:Class rdf:about="&android-2_3;AndroidContentRes">
		<rdfs:subClassOf rdf:resource="&android-2_2;AndroidContentRes"/>
		<rdfs:seeAlso rdf:resource="&android-2_3;AndroidGraphics"/>
		<rdfs:seeAlso rdf:resource="&android-2_3;JavaIo"/>
		<rdfs:seeAlso rdf:resource="&android-2_3;JavaLang"/>
		<rdfs:seeAlso rdf:resource="&android-2_3;AndroidGraphicsDrawable"/>
		<rdfs:seeAlso rdf:resource="&android-2_3;AndroidUtil"/>
		<rdfs:seeAlso rdf:resource="&android-2_3;JavaUtil"/>
		<rdfs:seeAlso rdf:resource="&android-2_3;AndroidOs"/>
		<rdfs:seeAlso rdf:resource="&android-2_3;OrgXmlpullV1"/>
		<rdfs:comment xml:lang="en">Java API part implementing the android.content.res package for Android 2.3</rdfs:comment>
	</owl:Class>
	<owl:Class rdf:about="&android-2_3;AndroidOs">
		<rdfs:subClassOf rdf:resource="&android-2_2;AndroidOs"/>
		<rdfs:seeAlso rdf:resource="&android-2_3;AndroidContent"/>
		<rdfs:seeAlso rdf:resource="&android-2_3;AndroidUtil"/>
		<rdfs:seeAlso rdf:resource="&android-2_3;JavaUtilConcurrent"/>
		<rdfs:seeAlso rdf:resource="&android-2_3;JavaIo"/>
		<rdfs:seeAlso rdf:resource="&android-2_3;JavaLang"/>
		<rdfs:seeAlso rdf:resource="&android-2_3;JavaNet"/>
		<rdfs:seeAlso rdf:resource="&android-2_3;JavaUtil"/>
		<rdfs:comment xml:lang="en">Java API part implementing the android.os package for Android 2.3</rdfs:comment>
	</owl:Class>
	<owl:Class rdf:about="&android-2_3;AndroidOsStorage">
		<rdfs:subClassOf rdf:resource="&java;JavaAPIPart"/>
		<rdfs:seeAlso rdf:resource="&android-2_3;JavaLang"/>
		<rdfs:comment xml:lang="en">Java API part implementing the android.os.storage package for Android 2.3</rdfs:comment>
	</owl:Class>
	<owl:Class rdf:about="&android-2_3;AndroidAccounts">
		<rdfs:subClassOf rdf:resource="&android-2_2;AndroidAccounts"/>
		<rdfs:seeAlso rdf:resource="&android-2_3;JavaUtilConcurrent"/>
		<rdfs:seeAlso rdf:resource="&android-2_3;AndroidContent"/>
		<rdfs:seeAlso rdf:resource="&android-2_3;JavaLang"/>
		<rdfs:seeAlso rdf:resource="&android-2_3;AndroidApp"/>
		<rdfs:seeAlso rdf:resource="&android-2_3;AndroidOs"/>
		<rdfs:comment xml:lang="en">Java API part implementing the android.accounts package for Android 2.3</rdfs:comment>
	</owl:Class>
	<owl:Class rdf:about="&android-2_3;AndroidNet">
		<rdfs:subClassOf rdf:resource="&android-2_2;AndroidNet"/>
		<rdfs:seeAlso rdf:resource="&android-2_3;JavaxNetSsl"/>
		<rdfs:seeAlso rdf:resource="&android-2_3;AndroidContent"/>
		<rdfs:seeAlso rdf:resource="&android-2_3;JavaIo"/>
		<rdfs:seeAlso rdf:resource="&android-2_3;JavaLang"/>
		<rdfs:seeAlso rdf:resource="&android-2_3;JavaNet"/>
		<rdfs:seeAlso rdf:resource="&android-2_3;JavaxNet"/>
		<rdfs:seeAlso rdf:resource="&android-2_3;OrgApacheHttpConnSsl"/>
		<rdfs:seeAlso rdf:resource="&android-2_3;JavaUtil"/>
		<rdfs:seeAlso rdf:resource="&android-2_3;AndroidOs"/>
		<rdfs:comment xml:lang="en">Java API part implementing the android.net package for Android 2.3</rdfs:comment>
	</owl:Class>
	<owl:Class rdf:about="&android-2_3;AndroidNetHttp">
		<owl:equivalentClass rdf:resource="&android-2_2;AndroidNetHttp"/>
		<rdfs:subClassOf rdf:resource="&java;JavaAPIPart"/>
		<rdfs:seeAlso rdf:resource="&android-2_3;OrgApacheHttpConn"/>
		<rdfs:seeAlso rdf:resource="&android-2_3;AndroidContent"/>
		<rdfs:seeAlso rdf:resource="&android-2_3;OrgApacheHttpEntity"/>
		<rdfs:seeAlso rdf:resource="&android-2_3;JavaIo"/>
		<rdfs:seeAlso rdf:resource="&android-2_3;JavaLang"/>
		<rdfs:seeAlso rdf:resource="&android-2_3;JavaSecurityCert"/>
		<rdfs:seeAlso rdf:resource="&android-2_3;OrgApacheHttpProtocol"/>
		<rdfs:seeAlso rdf:resource="&android-2_3;OrgApacheHttpClientMethods"/>
		<rdfs:seeAlso rdf:resource="&android-2_3;OrgApacheHttpParams"/>
		<rdfs:seeAlso rdf:resource="&android-2_3;AndroidOs"/>
		<rdfs:seeAlso rdf:resource="&android-2_3;JavaUtil"/>
		<rdfs:seeAlso rdf:resource="&android-2_3;OrgApacheHttp"/>
		<rdfs:seeAlso rdf:resource="&android-2_3;OrgApacheHttpClient"/>
		<rdfs:comment xml:lang="en">Java API part implementing the android.net.http package for Android 2.3</rdfs:comment>
	</owl:Class>
	<owl:Class rdf:about="&android-2_3;AndroidNetSip">
		<rdfs:subClassOf rdf:resource="&java;JavaAPIPart"/>
		<rdfs:seeAlso rdf:resource="&android-2_3;AndroidContent"/>
		<rdfs:seeAlso rdf:resource="&android-2_3;JavaIo"/>
		<rdfs:seeAlso rdf:resource="&android-2_3;JavaLang"/>
		<rdfs:seeAlso rdf:resource="&android-2_3;AndroidApp"/>
		<rdfs:seeAlso rdf:resource="&android-2_3;AndroidOs"/>
		<rdfs:comment xml:lang="en">Java API part implementing the android.net.sip package for Android 2.3</rdfs:comment>
	</owl:Class>
	<owl:Class rdf:about="&android-2_3;AndroidNetWifi">
		<rdfs:subClassOf rdf:resource="&android-2_2;AndroidNetWifi"/>
		<rdfs:seeAlso rdf:resource="&android-2_3;AndroidNet"/>
		<rdfs:seeAlso rdf:resource="&android-2_3;AndroidOs"/>
		<rdfs:seeAlso rdf:resource="&android-2_3;JavaUtil"/>
		<rdfs:seeAlso rdf:resource="&android-2_3;JavaLang"/>
		<rdfs:comment xml:lang="en">Java API part implementing the android.net.wifi package for Android 2.3</rdfs:comment>
	</owl:Class>
	<owl:Class rdf:about="&android-2_3;AndroidDatabase">
		<rdfs:subClassOf rdf:resource="&android-2_2;AndroidDatabase"/>
		<rdfs:seeAlso rdf:resource="&android-2_3;AndroidContent"/>
		<rdfs:seeAlso rdf:resource="&android-2_3;AndroidOs"/>
		<rdfs:seeAlso rdf:resource="&android-2_3;AndroidNet"/>
		<rdfs:seeAlso rdf:resource="&android-2_3;JavaIo"/>
		<rdfs:seeAlso rdf:resource="&android-2_3;JavaLang"/>
		<rdfs:seeAlso rdf:resource="&android-2_3;AndroidDatabaseSqlite"/>
		<rdfs:seeAlso rdf:resource="&android-2_3;JavaUtil"/>
		<rdfs:comment xml:lang="en">Java API part implementing the android.database package for Android 2.3</rdfs:comment>
	</owl:Class>
	<owl:Class rdf:about="&android-2_3;AndroidDatabaseSqlite">
		<owl:equivalentClass rdf:resource="&android-2_2;AndroidDatabaseSqlite"/>
		<rdfs:subClassOf rdf:resource="&java;JavaAPIPart"/>
		<rdfs:seeAlso rdf:resource="&android-2_3;AndroidContent"/>
		<rdfs:seeAlso rdf:resource="&android-2_3;JavaIo"/>
		<rdfs:seeAlso rdf:resource="&android-2_3;JavaLang"/>
		<rdfs:seeAlso rdf:resource="&android-2_3;JavaUtil"/>
		<rdfs:seeAlso rdf:resource="&android-2_3;AndroidDatabase"/>
		<rdfs:comment xml:lang="en">Java API part implementing the android.database.sqlite package for Android 2.3</rdfs:comment>
	</owl:Class>
	<owl:Class rdf:about="&android-2_3;AndroidUtil">
		<rdfs:subClassOf rdf:resource="&android-2_2;AndroidUtil"/>
		<rdfs:seeAlso rdf:resource="&android-2_3;OrgXmlSax"/>
		<rdfs:seeAlso rdf:resource="&android-2_3;JavaUtilRegex"/>
		<rdfs:seeAlso rdf:resource="&android-2_3;JavaIo"/>
		<rdfs:seeAlso rdf:resource="&android-2_3;JavaLang"/>
		<rdfs:seeAlso rdf:resource="&android-2_3;JavaUtil"/>
		<rdfs:seeAlso rdf:resource="&android-2_3;OrgXmlpullV1"/>
		<rdfs:comment xml:lang="en">Java API part implementing the android.util package for Android 2.3</rdfs:comment>
	</owl:Class>
	<owl:Class rdf:about="&android-2_3;AndroidGraphics">
		<rdfs:subClassOf rdf:resource="&android-2_2;AndroidGraphics"/>
		<rdfs:seeAlso rdf:resource="&android-2_3;JavaIo"/>
		<rdfs:seeAlso rdf:resource="&android-2_3;JavaLang"/>
		<rdfs:seeAlso rdf:resource="&android-2_3;JavaNio"/>
		<rdfs:seeAlso rdf:resource="&android-2_3;AndroidContentRes"/>
		<rdfs:seeAlso rdf:resource="&android-2_3;AndroidUtil"/>
		<rdfs:seeAlso rdf:resource="&android-2_3;AndroidOs"/>
		<rdfs:seeAlso rdf:resource="&android-2_3;JavaxMicroeditionKhronosOpengles"/>
		<rdfs:comment xml:lang="en">Java API part implementing the android.graphics package for Android 2.3</rdfs:comment>
	</owl:Class>
	<owl:Class rdf:about="&android-2_3;AndroidGraphicsDrawable">
		<rdfs:subClassOf rdf:resource="&android-2_2;AndroidGraphicsDrawable"/>
		<rdfs:seeAlso rdf:resource="&android-2_3;AndroidGraphics"/>
		<rdfs:seeAlso rdf:resource="&android-2_3;JavaIo"/>
		<rdfs:seeAlso rdf:resource="&android-2_3;JavaLang"/>
		<rdfs:seeAlso rdf:resource="&android-2_3;AndroidContentRes"/>
		<rdfs:seeAlso rdf:resource="&android-2_3;AndroidUtil"/>
		<rdfs:seeAlso rdf:resource="&android-2_3;OrgXmlpullV1"/>
		<rdfs:seeAlso rdf:resource="&android-2_3;AndroidGraphicsDrawableShapes"/>
		<rdfs:comment xml:lang="en">Java API part implementing the android.graphics.drawable package for Android 2.3</rdfs:comment>
	</owl:Class>
	<owl:Class rdf:about="&android-2_3;AndroidGraphicsDrawableShapes">
		<owl:equivalentClass rdf:resource="&android-2_2;AndroidGraphicsDrawableShapes"/>
		<rdfs:subClassOf rdf:resource="&java;JavaAPIPart"/>
		<rdfs:seeAlso rdf:resource="&android-2_3;AndroidGraphics"/>
		<rdfs:seeAlso rdf:resource="&android-2_3;JavaLang"/>
		<rdfs:comment xml:lang="en">Java API part implementing the android.graphics.drawable.shapes package for Android 2.3</rdfs:comment>
	</owl:Class>
	<owl:Class rdf:about="&android-2_3;AndroidView">
		<rdfs:subClassOf rdf:resource="&java;JavaAPIPart"/>
		<rdfs:seeAlso rdf:resource="&android-2_3;AndroidContent"/>
		<rdfs:seeAlso rdf:resource="&android-2_3;AndroidHardware"/>
		<rdfs:seeAlso rdf:resource="&android-2_3;AndroidContentRes"/>
		<rdfs:seeAlso rdf:resource="&android-2_3;AndroidUtil"/>
		<rdfs:seeAlso rdf:resource="&android-2_3;AndroidOs"/>
		<rdfs:seeAlso rdf:resource="&android-2_3;AndroidViewAnimation"/>
		<rdfs:seeAlso rdf:resource="&android-2_3;AndroidGraphics"/>
		<rdfs:seeAlso rdf:resource="&android-2_3;AndroidViewInputmethod"/>
		<rdfs:seeAlso rdf:resource="&android-2_3;AndroidNet"/>
		<rdfs:seeAlso rdf:resource="&android-2_3;AndroidViewAccessibility"/>
		<rdfs:seeAlso rdf:resource="&android-2_3;JavaLang"/>
		<rdfs:seeAlso rdf:resource="&android-2_3;JavaLangAnnotation"/>
		<rdfs:seeAlso rdf:resource="&android-2_3;AndroidGraphicsDrawable"/>
		<rdfs:seeAlso rdf:resource="&android-2_3;JavaUtil"/>
		<rdfs:seeAlso rdf:resource="&android-2_3;OrgXmlpullV1"/>
		<rdfs:comment xml:lang="en">Java API part implementing the android.view package for Android 2.3</rdfs:comment>
	</owl:Class>
	<owl:Class rdf:about="&android-2_3;AndroidViewAccessibility">
		<owl:equivalentClass rdf:resource="&android-2_2;AndroidViewAccessibility"/>
		<rdfs:subClassOf rdf:resource="&java;JavaAPIPart"/>
		<rdfs:seeAlso rdf:resource="&android-2_3;JavaUtil"/>
		<rdfs:seeAlso rdf:resource="&android-2_3;AndroidOs"/>
		<rdfs:seeAlso rdf:resource="&android-2_3;JavaLang"/>
		<rdfs:comment xml:lang="en">Java API part implementing the android.view.accessibility package for Android 2.3</rdfs:comment>
	</owl:Class>
	<owl:Class rdf:about="&android-2_3;AndroidViewInputmethod">
		<rdfs:subClassOf rdf:resource="&android-2_2;AndroidViewInputmethod"/>
		<rdfs:seeAlso rdf:resource="&android-2_3;AndroidView"/>
		<rdfs:seeAlso rdf:resource="&android-2_3;AndroidContent"/>
		<rdfs:seeAlso rdf:resource="&android-2_3;AndroidText"/>
		<rdfs:seeAlso rdf:resource="&android-2_3;AndroidUtil"/>
		<rdfs:seeAlso rdf:resource="&android-2_3;AndroidOs"/>
		<rdfs:seeAlso rdf:resource="&android-2_3;AndroidContentPm"/>
		<rdfs:seeAlso rdf:resource="&android-2_3;AndroidGraphics"/>
		<rdfs:seeAlso rdf:resource="&android-2_3;JavaLang"/>
		<rdfs:seeAlso rdf:resource="&android-2_3;AndroidGraphicsDrawable"/>
		<rdfs:seeAlso rdf:resource="&android-2_3;JavaUtil"/>
		<rdfs:comment xml:lang="en">Java API part implementing the android.view.inputmethod package for Android 2.3</rdfs:comment>
	</owl:Class>
	<owl:Class rdf:about="&android-2_3;AndroidViewAnimation">
		<owl:equivalentClass rdf:resource="&android-2_2;AndroidViewAnimation"/>
		<rdfs:subClassOf rdf:resource="&java;JavaAPIPart"/>
		<rdfs:seeAlso rdf:resource="&android-2_3;AndroidView"/>
		<rdfs:seeAlso rdf:resource="&android-2_3;AndroidGraphics"/>
		<rdfs:seeAlso rdf:resource="&android-2_3;AndroidUtil"/>
		<rdfs:seeAlso rdf:resource="&android-2_3;AndroidContent"/>
		<rdfs:seeAlso rdf:resource="&android-2_3;JavaUtil"/>
		<rdfs:seeAlso rdf:resource="&android-2_3;JavaLang"/>
		<rdfs:comment xml:lang="en">Java API part implementing the android.view.animation package for Android 2.3</rdfs:comment>
	</owl:Class>
	<owl:Class rdf:about="&android-2_3;AndroidAccessibilityservice">
		<rdfs:subClassOf rdf:resource="&android-2_2;AndroidAccessibilityservice"/>
		<rdfs:seeAlso rdf:resource="&android-2_3;AndroidApp"/>
		<rdfs:seeAlso rdf:resource="&android-2_3;AndroidContent"/>
		<rdfs:seeAlso rdf:resource="&android-2_3;AndroidViewAccessibility"/>
		<rdfs:seeAlso rdf:resource="&android-2_3;AndroidOs"/>
		<rdfs:seeAlso rdf:resource="&android-2_3;JavaLang"/>
		<rdfs:comment xml:lang="en">Java API part implementing the android.accessibilityservice package for Android 2.3</rdfs:comment>
	</owl:Class>
	<owl:Class rdf:about="&android-2_3;AndroidApp">
		<rdfs:subClassOf rdf:resource="&android-2_2;AndroidApp"/>
		<rdfs:seeAlso rdf:resource="&android-2_3;AndroidView"/>
		<rdfs:seeAlso rdf:resource="&android-2_3;AndroidContent"/>
		<rdfs:seeAlso rdf:resource="&android-2_3;AndroidUtil"/>
		<rdfs:seeAlso rdf:resource="&android-2_3;AndroidNet"/>
		<rdfs:seeAlso rdf:resource="&android-2_3;AndroidDatabase"/>
		<rdfs:seeAlso rdf:resource="&android-2_3;AndroidContentRes"/>
		<rdfs:seeAlso rdf:resource="&android-2_3;AndroidWidget"/>
		<rdfs:seeAlso rdf:resource="&android-2_3;AndroidOs"/>
		<rdfs:seeAlso rdf:resource="&android-2_3;AndroidContentPm"/>
		<rdfs:seeAlso rdf:resource="&android-2_3;AndroidGraphics"/>
		<rdfs:seeAlso rdf:resource="&android-2_3;AndroidViewAccessibility"/>
		<rdfs:seeAlso rdf:resource="&android-2_3;JavaIo"/>
		<rdfs:seeAlso rdf:resource="&android-2_3;JavaLang"/>
		<rdfs:seeAlso rdf:resource="&android-2_3;AndroidGraphicsDrawable"/>
		<rdfs:seeAlso rdf:resource="&android-2_3;JavaUtil"/>
		<rdfs:comment xml:lang="en">Java API part implementing the android.app package for Android 2.3</rdfs:comment>
	</owl:Class>
	<owl:Class rdf:about="&android-2_3;AndroidAppBackup">
		<rdfs:subClassOf rdf:resource="&android-2_2;AndroidAppBackup"/>
		<rdfs:seeAlso rdf:resource="&android-2_3;AndroidOs"/>
		<rdfs:seeAlso rdf:resource="&android-2_3;AndroidContent"/>
		<rdfs:seeAlso rdf:resource="&android-2_3;JavaIo"/>
		<rdfs:seeAlso rdf:resource="&android-2_3;JavaLang"/>
		<rdfs:comment xml:lang="en">Java API part implementing the android.app.backup package for Android 2.3</rdfs:comment>
	</owl:Class>
	<owl:Class rdf:about="&android-2_3;AndroidAppAdmin">
		<rdfs:subClassOf rdf:resource="&android-2_2;AndroidAppAdmin"/>
		<rdfs:seeAlso rdf:resource="&android-2_3;AndroidContent"/>
		<rdfs:seeAlso rdf:resource="&android-2_3;JavaLang"/>
		<rdfs:seeAlso rdf:resource="&android-2_3;AndroidGraphicsDrawable"/>
		<rdfs:seeAlso rdf:resource="&android-2_3;AndroidUtil"/>
		<rdfs:seeAlso rdf:resource="&android-2_3;JavaUtil"/>
		<rdfs:seeAlso rdf:resource="&android-2_3;AndroidOs"/>
		<rdfs:seeAlso rdf:resource="&android-2_3;AndroidContentPm"/>
		<rdfs:comment xml:lang="en">Java API part implementing the android.app.admin package for Android 2.3</rdfs:comment>
	</owl:Class>
	<owl:Class rdf:about="&android-2_3;AndroidTelephony">
		<rdfs:subClassOf rdf:resource="&android-2_2;AndroidTelephony"/>
		<rdfs:seeAlso rdf:resource="&android-2_3;AndroidContent"/>
		<rdfs:seeAlso rdf:resource="&android-2_3;JavaLang"/>
		<rdfs:seeAlso rdf:resource="&android-2_3;AndroidText"/>
		<rdfs:seeAlso rdf:resource="&android-2_3;AndroidApp"/>
		<rdfs:seeAlso rdf:resource="&android-2_3;JavaUtil"/>
		<rdfs:seeAlso rdf:resource="&android-2_3;AndroidOs"/>
		<rdfs:comment xml:lang="en">Java API part implementing the android.telephony package for Android 2.3</rdfs:comment>
	</owl:Class>
	<owl:Class rdf:about="&android-2_3;AndroidTelephonyCdma">
		<owl:equivalentClass rdf:resource="&android-2_2;AndroidTelephonyCdma"/>
		<rdfs:subClassOf rdf:resource="&java;JavaAPIPart"/>
		<rdfs:seeAlso rdf:resource="&android-2_3;AndroidTelephony"/>
		<rdfs:seeAlso rdf:resource="&android-2_3;AndroidOs"/>
		<rdfs:seeAlso rdf:resource="&android-2_3;JavaLang"/>
		<rdfs:comment xml:lang="en">Java API part implementing the android.telephony.cdma package for Android 2.3</rdfs:comment>
	</owl:Class>
	<owl:Class rdf:about="&android-2_3;AndroidTelephonyGsm">
		<rdfs:subClassOf rdf:resource="&android-2_2;AndroidTelephonyGsm"/>
		<rdfs:seeAlso rdf:resource="&android-2_3;AndroidApp"/>
		<rdfs:seeAlso rdf:resource="&android-2_3;AndroidTelephony"/>
		<rdfs:seeAlso rdf:resource="&android-2_3;JavaUtil"/>
		<rdfs:seeAlso rdf:resource="&android-2_3;AndroidOs"/>
		<rdfs:seeAlso rdf:resource="&android-2_3;JavaLang"/>
		<rdfs:comment xml:lang="en">Java API part implementing the android.telephony.gsm package for Android 2.3</rdfs:comment>
	</owl:Class>
	<owl:Class rdf:about="&android-2_3;AndroidText">
		<rdfs:subClassOf rdf:resource="&android-2_2;AndroidText"/>
		<rdfs:seeAlso rdf:resource="&android-2_3;OrgXmlSax"/>
		<rdfs:seeAlso rdf:resource="&android-2_3;AndroidView"/>
		<rdfs:seeAlso rdf:resource="&android-2_3;AndroidGraphics"/>
		<rdfs:seeAlso rdf:resource="&android-2_3;JavaUtilRegex"/>
		<rdfs:seeAlso rdf:resource="&android-2_3;JavaLang"/>
		<rdfs:seeAlso rdf:resource="&android-2_3;AndroidGraphicsDrawable"/>
		<rdfs:seeAlso rdf:resource="&android-2_3;AndroidUtil"/>
		<rdfs:seeAlso rdf:resource="&android-2_3;AndroidOs"/>
		<rdfs:seeAlso rdf:resource="&android-2_3;JavaUtil"/>
		<rdfs:comment xml:lang="en">Java API part implementing the android.text package for Android 2.3</rdfs:comment>
	</owl:Class>
	<owl:Class rdf:about="&android-2_3;AndroidTextUtil">
		<owl:equivalentClass rdf:resource="&android-2_2;AndroidTextUtil"/>
		<rdfs:subClassOf rdf:resource="&java;JavaAPIPart"/>
		<rdfs:seeAlso rdf:resource="&android-2_3;AndroidWidget"/>
		<rdfs:seeAlso rdf:resource="&android-2_3;JavaUtilRegex"/>
		<rdfs:seeAlso rdf:resource="&android-2_3;JavaUtil"/>
		<rdfs:seeAlso rdf:resource="&android-2_3;JavaLang"/>
		<rdfs:seeAlso rdf:resource="&android-2_3;AndroidText"/>
		<rdfs:comment xml:lang="en">Java API part implementing the android.text.util package for Android 2.3</rdfs:comment>
	</owl:Class>
	<owl:Class rdf:about="&android-2_3;AndroidTextFormat">
		<rdfs:subClassOf rdf:resource="&android-2_2;AndroidTextFormat"/>
		<rdfs:seeAlso rdf:resource="&android-2_3;JavaText"/>
		<rdfs:seeAlso rdf:resource="&android-2_3;AndroidContent"/>
		<rdfs:seeAlso rdf:resource="&android-2_3;JavaUtil"/>
		<rdfs:seeAlso rdf:resource="&android-2_3;JavaLang"/>
		<rdfs:comment xml:lang="en">Java API part implementing the android.text.format package for Android 2.3</rdfs:comment>
	</owl:Class>
	<owl:Class rdf:about="&android-2_3;AndroidTextMethod">
		<rdfs:subClassOf rdf:resource="&android-2_2;AndroidTextMethod"/>
		<rdfs:seeAlso rdf:resource="&android-2_3;AndroidView"/>
		<rdfs:seeAlso rdf:resource="&android-2_3;AndroidGraphics"/>
		<rdfs:seeAlso rdf:resource="&android-2_3;AndroidContent"/>
		<rdfs:seeAlso rdf:resource="&android-2_3;JavaLang"/>
		<rdfs:seeAlso rdf:resource="&android-2_3;AndroidText"/>
		<rdfs:seeAlso rdf:resource="&android-2_3;AndroidApp"/>
		<rdfs:seeAlso rdf:resource="&android-2_3;AndroidWidget"/>
		<rdfs:seeAlso rdf:resource="&android-2_3;AndroidOs"/>
		<rdfs:comment xml:lang="en">Java API part implementing the android.text.method package for Android 2.3</rdfs:comment>
	</owl:Class>
	<owl:Class rdf:about="&android-2_3;AndroidTextStyle">
		<owl:equivalentClass rdf:resource="&android-2_2;AndroidTextStyle"/>
		<rdfs:subClassOf rdf:resource="&java;JavaAPIPart"/>
		<rdfs:seeAlso rdf:resource="&android-2_3;AndroidView"/>
		<rdfs:seeAlso rdf:resource="&android-2_3;AndroidGraphics"/>
		<rdfs:seeAlso rdf:resource="&android-2_3;AndroidNet"/>
		<rdfs:seeAlso rdf:resource="&android-2_3;AndroidContent"/>
		<rdfs:seeAlso rdf:resource="&android-2_3;JavaLang"/>
		<rdfs:seeAlso rdf:resource="&android-2_3;AndroidText"/>
		<rdfs:seeAlso rdf:resource="&android-2_3;AndroidGraphicsDrawable"/>
		<rdfs:seeAlso rdf:resource="&android-2_3;AndroidContentRes"/>
		<rdfs:seeAlso rdf:resource="&android-2_3;AndroidOs"/>
		<rdfs:comment xml:lang="en">Java API part implementing the android.text.style package for Android 2.3</rdfs:comment>
	</owl:Class>
	<owl:Class rdf:about="&android-2_3;AndroidGesture">
		<rdfs:subClassOf rdf:resource="&android-2_2;AndroidGesture"/>
		<rdfs:seeAlso rdf:resource="&android-2_3;AndroidView"/>
		<rdfs:seeAlso rdf:resource="&android-2_3;AndroidGraphics"/>
		<rdfs:seeAlso rdf:resource="&android-2_3;AndroidContent"/>
		<rdfs:seeAlso rdf:resource="&android-2_3;JavaIo"/>
		<rdfs:seeAlso rdf:resource="&android-2_3;JavaLang"/>
		<rdfs:seeAlso rdf:resource="&android-2_3;AndroidUtil"/>
		<rdfs:seeAlso rdf:resource="&android-2_3;AndroidWidget"/>
		<rdfs:seeAlso rdf:resource="&android-2_3;JavaUtil"/>
		<rdfs:seeAlso rdf:resource="&android-2_3;AndroidOs"/>
		<rdfs:comment xml:lang="en">Java API part implementing the android.gesture package for Android 2.3</rdfs:comment>
	</owl:Class>
	<owl:Class rdf:about="&android-2_3;AndroidWidget">
		<rdfs:subClassOf rdf:resource="&android-2_2;AndroidWidget"/>
		<rdfs:seeAlso rdf:resource="&android-2_3;AndroidView"/>
		<rdfs:seeAlso rdf:resource="&android-2_3;AndroidContent"/>
		<rdfs:seeAlso rdf:resource="&android-2_3;AndroidText"/>
		<rdfs:seeAlso rdf:resource="&android-2_3;AndroidUtil"/>
		<rdfs:seeAlso rdf:resource="&android-2_3;AndroidNet"/>
		<rdfs:seeAlso rdf:resource="&android-2_3;AndroidViewInputmethod"/>
		<rdfs:seeAlso rdf:resource="&android-2_3;JavaLangAnnotation"/>
		<rdfs:seeAlso rdf:resource="&android-2_3;AndroidTextMethod"/>
		<rdfs:seeAlso rdf:resource="&android-2_3;AndroidMedia"/>
		<rdfs:seeAlso rdf:resource="&android-2_3;AndroidDatabase"/>
		<rdfs:seeAlso rdf:resource="&android-2_3;AndroidContentRes"/>
		<rdfs:seeAlso rdf:resource="&android-2_3;AndroidApp"/>
		<rdfs:seeAlso rdf:resource="&android-2_3;AndroidOs"/>
		<rdfs:seeAlso rdf:resource="&android-2_3;AndroidViewAnimation"/>
		<rdfs:seeAlso rdf:resource="&android-2_3;AndroidGraphics"/>
		<rdfs:seeAlso rdf:resource="&android-2_3;AndroidViewAccessibility"/>
		<rdfs:seeAlso rdf:resource="&android-2_3;JavaLang"/>
		<rdfs:seeAlso rdf:resource="&android-2_3;AndroidGraphicsDrawable"/>
		<rdfs:seeAlso rdf:resource="&android-2_3;JavaUtil"/>
		<rdfs:comment xml:lang="en">Java API part implementing the android.widget package for Android 2.3</rdfs:comment>
	</owl:Class>
	<owl:Class rdf:about="&android-2_3;AndroidLocation">
		<rdfs:subClassOf rdf:resource="&android-2_2;AndroidLocation"/>
		<rdfs:seeAlso rdf:resource="&android-2_3;AndroidContent"/>
		<rdfs:seeAlso rdf:resource="&android-2_3;JavaLang"/>
		<rdfs:seeAlso rdf:resource="&android-2_3;AndroidApp"/>
		<rdfs:seeAlso rdf:resource="&android-2_3;AndroidUtil"/>
		<rdfs:seeAlso rdf:resource="&android-2_3;JavaUtil"/>
		<rdfs:seeAlso rdf:resource="&android-2_3;AndroidOs"/>
		<rdfs:comment xml:lang="en">Java API part implementing the android.location package for Android 2.3</rdfs:comment>
	</owl:Class>
	<owl:Class rdf:about="&android-2_3;AndroidHardware">
		<rdfs:subClassOf rdf:resource="&android-2_2;AndroidHardware"/>
		<rdfs:seeAlso rdf:resource="&android-2_3;AndroidView"/>
		<rdfs:seeAlso rdf:resource="&android-2_3;AndroidOs"/>
		<rdfs:seeAlso rdf:resource="&android-2_3;JavaUtil"/>
		<rdfs:seeAlso rdf:resource="&android-2_3;JavaLang"/>
		<rdfs:comment xml:lang="en">Java API part implementing the android.hardware package for Android 2.3</rdfs:comment>
	</owl:Class>
	<owl:Class rdf:about="&android-2_3;AndroidWebkit">
		<rdfs:subClassOf rdf:resource="&android-2_2;AndroidWebkit"/>
		<rdfs:seeAlso rdf:resource="&android-2_3;AndroidView"/>
		<rdfs:seeAlso rdf:resource="&android-2_3;AndroidContent"/>
		<rdfs:seeAlso rdf:resource="&android-2_3;AndroidNetHttp"/>
		<rdfs:seeAlso rdf:resource="&android-2_3;AndroidWidget"/>
		<rdfs:seeAlso rdf:resource="&android-2_3;AndroidUtil"/>
		<rdfs:seeAlso rdf:resource="&android-2_3;AndroidOs"/>
		<rdfs:seeAlso rdf:resource="&android-2_3;AndroidGraphics"/>
		<rdfs:seeAlso rdf:resource="&android-2_3;AndroidViewInputmethod"/>
		<rdfs:seeAlso rdf:resource="&android-2_3;JavaIo"/>
		<rdfs:seeAlso rdf:resource="&android-2_3;JavaLang"/>
		<rdfs:seeAlso rdf:resource="&android-2_3;JavaUtil"/>
		<rdfs:comment xml:lang="en">Java API part implementing the android.webkit package for Android 2.3</rdfs:comment>
	</owl:Class>
	<owl:Class rdf:about="&android-2_3;AndroidTest">
		<rdfs:subClassOf rdf:resource="&android-2_2;AndroidTest"/>
		<rdfs:seeAlso rdf:resource="&android-2_3;AndroidView"/>
		<rdfs:seeAlso rdf:resource="&android-2_3;AndroidContent"/>
		<rdfs:seeAlso rdf:resource="&android-2_3;AndroidTestMock"/>
		<rdfs:seeAlso rdf:resource="&android-2_3;AndroidApp"/>
		<rdfs:seeAlso rdf:resource="&android-2_3;AndroidOs"/>
		<rdfs:seeAlso rdf:resource="&android-2_3;AndroidNet"/>
		<rdfs:seeAlso rdf:resource="&android-2_3;JunitRunner"/>
		<rdfs:seeAlso rdf:resource="&android-2_3;JavaUtilRegex"/>
		<rdfs:seeAlso rdf:resource="&android-2_3;JavaIo"/>
		<rdfs:seeAlso rdf:resource="&android-2_3;JavaLang"/>
		<rdfs:seeAlso rdf:resource="&android-2_3;AndroidDatabaseSqlite"/>
		<rdfs:seeAlso rdf:resource="&android-2_3;JavaLangAnnotation"/>
		<rdfs:seeAlso rdf:resource="&android-2_3;JunitFramework"/>
		<rdfs:seeAlso rdf:resource="&android-2_3;JavaUtil"/>
		<rdfs:comment xml:lang="en">Java API part implementing the android.test package for Android 2.3</rdfs:comment>
	</owl:Class>
	<owl:Class rdf:about="&android-2_3;AndroidTestMock">
		<rdfs:subClassOf rdf:resource="&android-2_2;AndroidTestMock"/>
		<rdfs:seeAlso rdf:resource="&android-2_3;AndroidContent"/>
		<rdfs:seeAlso rdf:resource="&android-2_3;AndroidUtil"/>
		<rdfs:seeAlso rdf:resource="&android-2_3;AndroidNet"/>
		<rdfs:seeAlso rdf:resource="&android-2_3;AndroidDatabase"/>
		<rdfs:seeAlso rdf:resource="&android-2_3;AndroidApp"/>
		<rdfs:seeAlso rdf:resource="&android-2_3;AndroidContentRes"/>
		<rdfs:seeAlso rdf:resource="&android-2_3;AndroidOs"/>
		<rdfs:seeAlso rdf:resource="&android-2_3;AndroidContentPm"/>
		<rdfs:seeAlso rdf:resource="&android-2_3;AndroidGraphics"/>
		<rdfs:seeAlso rdf:resource="&android-2_3;JavaIo"/>
		<rdfs:seeAlso rdf:resource="&android-2_3;JavaLang"/>
		<rdfs:seeAlso rdf:resource="&android-2_3;AndroidDatabaseSqlite"/>
		<rdfs:seeAlso rdf:resource="&android-2_3;AndroidGraphicsDrawable"/>
		<rdfs:seeAlso rdf:resource="&android-2_3;JavaUtil"/>
		<rdfs:comment xml:lang="en">Java API part implementing the android.test.mock package for Android 2.3</rdfs:comment>
	</owl:Class>
	<owl:Class rdf:about="&android-2_3;AndroidTestSuitebuilder">
		<owl:equivalentClass rdf:resource="&android-2_2;AndroidTestSuitebuilder"/>
		<rdfs:subClassOf rdf:resource="&java;JavaAPIPart"/>
		<rdfs:seeAlso rdf:resource="&android-2_3;JunitFramework"/>
		<rdfs:seeAlso rdf:resource="&android-2_3;JavaLangReflect"/>
		<rdfs:seeAlso rdf:resource="&android-2_3;JavaUtil"/>
		<rdfs:seeAlso rdf:resource="&android-2_3;JavaLang"/>
		<rdfs:seeAlso rdf:resource="&android-2_3;JavaLangAnnotation"/>
		<rdfs:comment xml:lang="en">Java API part implementing the android.test.suitebuilder package for Android 2.3</rdfs:comment>
	</owl:Class>
	<owl:Class rdf:about="&android-2_3;AndroidTestSuitebuilderAnnotation">
		<owl:equivalentClass rdf:resource="&android-2_2;AndroidTestSuitebuilderAnnotation"/>
		<rdfs:subClassOf rdf:resource="&java;JavaAPIPart"/>
		<rdfs:seeAlso rdf:resource="&android-2_3;JavaLangAnnotation"/>
		<rdfs:comment xml:lang="en">Java API part implementing the android.test.suitebuilder.annotation package for Android 2.3</rdfs:comment>
	</owl:Class>
	<owl:Class rdf:about="&android-2_3;AndroidPreference">
		<rdfs:subClassOf rdf:resource="&android-2_2;AndroidPreference"/>
		<rdfs:seeAlso rdf:resource="&android-2_3;AndroidView"/>
		<rdfs:seeAlso rdf:resource="&android-2_3;AndroidContent"/>
		<rdfs:seeAlso rdf:resource="&android-2_3;AndroidContentRes"/>
		<rdfs:seeAlso rdf:resource="&android-2_3;AndroidApp"/>
		<rdfs:seeAlso rdf:resource="&android-2_3;AndroidUtil"/>
		<rdfs:seeAlso rdf:resource="&android-2_3;AndroidWidget"/>
		<rdfs:seeAlso rdf:resource="&android-2_3;AndroidOs"/>
		<rdfs:seeAlso rdf:resource="&android-2_3;AndroidNet"/>
		<rdfs:seeAlso rdf:resource="&android-2_3;JavaLang"/>
		<rdfs:seeAlso rdf:resource="&android-2_3;AndroidGraphicsDrawable"/>
		<rdfs:comment xml:lang="en">Java API part implementing the android.preference package for Android 2.3</rdfs:comment>
	</owl:Class>
	<owl:Class rdf:about="&android-2_3;AndroidMedia">
		<rdfs:subClassOf rdf:resource="&android-2_2;AndroidMedia"/>
		<rdfs:seeAlso rdf:resource="&android-2_3;AndroidView"/>
		<rdfs:seeAlso rdf:resource="&android-2_3;AndroidGraphics"/>
		<rdfs:seeAlso rdf:resource="&android-2_3;AndroidNet"/>
		<rdfs:seeAlso rdf:resource="&android-2_3;AndroidContent"/>
		<rdfs:seeAlso rdf:resource="&android-2_3;JavaIo"/>
		<rdfs:seeAlso rdf:resource="&android-2_3;JavaLang"/>
		<rdfs:seeAlso rdf:resource="&android-2_3;AndroidHardware"/>
		<rdfs:seeAlso rdf:resource="&android-2_3;JavaNio"/>
		<rdfs:seeAlso rdf:resource="&android-2_3;AndroidApp"/>
		<rdfs:seeAlso rdf:resource="&android-2_3;AndroidContentRes"/>
		<rdfs:seeAlso rdf:resource="&android-2_3;AndroidOs"/>
		<rdfs:seeAlso rdf:resource="&android-2_3;AndroidDatabase"/>
		<rdfs:comment xml:lang="en">Java API part implementing the android.media package for Android 2.3</rdfs:comment>
	</owl:Class>
	<owl:Class rdf:about="&android-2_3;AndroidMediaAudiofx">
		<rdfs:subClassOf rdf:resource="&java;JavaAPIPart"/>
		<rdfs:seeAlso rdf:resource="&android-2_3;JavaUtil"/>
		<rdfs:seeAlso rdf:resource="&android-2_3;JavaLang"/>
		<rdfs:comment xml:lang="en">Java API part implementing the android.media.audiofx package for Android 2.3</rdfs:comment>
	</owl:Class>
	<owl:Class rdf:about="&android-2_3;AndroidInputmethodservice">
		<rdfs:subClassOf rdf:resource="&android-2_2;AndroidInputmethodservice"/>
		<rdfs:seeAlso rdf:resource="&android-2_3;AndroidView"/>
		<rdfs:seeAlso rdf:resource="&android-2_3;AndroidContent"/>
		<rdfs:seeAlso rdf:resource="&android-2_3;AndroidApp"/>
		<rdfs:seeAlso rdf:resource="&android-2_3;AndroidContentRes"/>
		<rdfs:seeAlso rdf:resource="&android-2_3;AndroidUtil"/>
		<rdfs:seeAlso rdf:resource="&android-2_3;AndroidWidget"/>
		<rdfs:seeAlso rdf:resource="&android-2_3;AndroidOs"/>
		<rdfs:seeAlso rdf:resource="&android-2_3;AndroidGraphics"/>
		<rdfs:seeAlso rdf:resource="&android-2_3;AndroidViewInputmethod"/>
		<rdfs:seeAlso rdf:resource="&android-2_3;JavaIo"/>
		<rdfs:seeAlso rdf:resource="&android-2_3;JavaLang"/>
		<rdfs:seeAlso rdf:resource="&android-2_3;AndroidGraphicsDrawable"/>
		<rdfs:seeAlso rdf:resource="&android-2_3;JavaUtil"/>
		<rdfs:comment xml:lang="en">Java API part implementing the android.inputmethodservice package for Android 2.3</rdfs:comment>
	</owl:Class>
	<owl:Class rdf:about="&android-2_3;AndroidServiceWallpaper">
		<rdfs:subClassOf rdf:resource="&android-2_2;AndroidServiceWallpaper"/>
		<rdfs:seeAlso rdf:resource="&android-2_3;AndroidView"/>
		<rdfs:seeAlso rdf:resource="&android-2_3;AndroidApp"/>
		<rdfs:seeAlso rdf:resource="&android-2_3;AndroidContent"/>
		<rdfs:seeAlso rdf:resource="&android-2_3;AndroidOs"/>
		<rdfs:seeAlso rdf:resource="&android-2_3;JavaLang"/>
		<rdfs:comment xml:lang="en">Java API part implementing the android.service.wallpaper package for Android 2.3</rdfs:comment>
	</owl:Class>
	<owl:Class rdf:about="&android-2_3;AndroidBluetooth">
		<owl:equivalentClass rdf:resource="&android-2_2;AndroidBluetooth"/>
		<rdfs:subClassOf rdf:resource="&java;JavaAPIPart"/>
		<rdfs:seeAlso rdf:resource="&android-2_3;JavaUtil"/>
		<rdfs:seeAlso rdf:resource="&android-2_3;AndroidOs"/>
		<rdfs:seeAlso rdf:resource="&android-2_3;JavaIo"/>
		<rdfs:seeAlso rdf:resource="&android-2_3;JavaLang"/>
		<rdfs:comment xml:lang="en">Java API part implementing the android.bluetooth package for Android 2.3</rdfs:comment>
	</owl:Class>
	<owl:Class rdf:about="&android-2_3;AndroidNfc">
		<rdfs:subClassOf rdf:resource="&java;JavaAPIPart"/>
		<rdfs:seeAlso rdf:resource="&android-2_3;AndroidOs"/>
		<rdfs:seeAlso rdf:resource="&android-2_3;JavaLang"/>
		<rdfs:comment xml:lang="en">Java API part implementing the android.nfc package for Android 2.3</rdfs:comment>
	</owl:Class>
	<owl:Class rdf:about="&android-2_3;AndroidProvider">
		<rdfs:subClassOf rdf:resource="&android-2_2;AndroidProvider"/>
		<rdfs:seeAlso rdf:resource="&android-2_3;AndroidView"/>
		<rdfs:seeAlso rdf:resource="&android-2_3;AndroidGraphics"/>
		<rdfs:seeAlso rdf:resource="&android-2_3;AndroidNet"/>
		<rdfs:seeAlso rdf:resource="&android-2_3;AndroidContent"/>
		<rdfs:seeAlso rdf:resource="&android-2_3;JavaIo"/>
		<rdfs:seeAlso rdf:resource="&android-2_3;JavaLang"/>
		<rdfs:seeAlso rdf:resource="&android-2_3;AndroidAccounts"/>
		<rdfs:seeAlso rdf:resource="&android-2_3;AndroidContentRes"/>
		<rdfs:seeAlso rdf:resource="&android-2_3;AndroidWebkit"/>
		<rdfs:seeAlso rdf:resource="&android-2_3;AndroidUtil"/>
		<rdfs:seeAlso rdf:resource="&android-2_3;AndroidDatabase"/>
		<rdfs:comment xml:lang="en">Java API part implementing the android.provider package for Android 2.3</rdfs:comment>
	</owl:Class>
	<owl:Class rdf:about="&android-2_3;AndroidSax">
		<owl:equivalentClass rdf:resource="&android-2_2;AndroidSax"/>
		<rdfs:subClassOf rdf:resource="&java;JavaAPIPart"/>
		<rdfs:seeAlso rdf:resource="&android-2_3;OrgXmlSax"/>
		<rdfs:seeAlso rdf:resource="&android-2_3;JavaLang"/>
		<rdfs:comment xml:lang="en">Java API part implementing the android.sax package for Android 2.3</rdfs:comment>
	</owl:Class>
	<owl:Class rdf:about="&android-2_3;AndroidAppwidget">
		<rdfs:subClassOf rdf:resource="&android-2_2;AndroidAppwidget"/>
		<rdfs:seeAlso rdf:resource="&android-2_3;AndroidView"/>
		<rdfs:seeAlso rdf:resource="&android-2_3;AndroidGraphics"/>
		<rdfs:seeAlso rdf:resource="&android-2_3;AndroidContent"/>
		<rdfs:seeAlso rdf:resource="&android-2_3;JavaLang"/>
		<rdfs:seeAlso rdf:resource="&android-2_3;AndroidUtil"/>
		<rdfs:seeAlso rdf:resource="&android-2_3;AndroidWidget"/>
		<rdfs:seeAlso rdf:resource="&android-2_3;JavaUtil"/>
		<rdfs:seeAlso rdf:resource="&android-2_3;AndroidOs"/>
		<rdfs:comment xml:lang="en">Java API part implementing the android.appwidget package for Android 2.3</rdfs:comment>
	</owl:Class>
	<owl:Class rdf:about="&android-2_3;AndroidOpengl">
		<rdfs:subClassOf rdf:resource="&android-2_2;AndroidOpengl"/>
		<rdfs:seeAlso rdf:resource="&android-2_3;AndroidView"/>
		<rdfs:seeAlso rdf:resource="&android-2_3;AndroidContent"/>
		<rdfs:seeAlso rdf:resource="&android-2_3;JavaNio"/>
		<rdfs:seeAlso rdf:resource="&android-2_3;AndroidUtil"/>
		<rdfs:seeAlso rdf:resource="&android-2_3;AndroidGraphics"/>
		<rdfs:seeAlso rdf:resource="&android-2_3;JavaIo"/>
		<rdfs:seeAlso rdf:resource="&android-2_3;JavaLang"/>
		<rdfs:seeAlso rdf:resource="&android-2_3;JavaxMicroeditionKhronosEgl"/>
		<rdfs:seeAlso rdf:resource="&android-2_3;JavaxMicroeditionKhronosOpengles"/>
		<rdfs:comment xml:lang="en">Java API part implementing the android.opengl package for Android 2.3</rdfs:comment>
	</owl:Class>
	<owl:Class rdf:about="&android-2_3;AndroidSpeech">
		<rdfs:subClassOf rdf:resource="&android-2_2;AndroidSpeech"/>
		<rdfs:seeAlso rdf:resource="&android-2_3;AndroidApp"/>
		<rdfs:seeAlso rdf:resource="&android-2_3;AndroidOs"/>
		<rdfs:seeAlso rdf:resource="&android-2_3;AndroidContent"/>
		<rdfs:seeAlso rdf:resource="&android-2_3;JavaLang"/>
		<rdfs:comment xml:lang="en">Java API part implementing the android.speech package for Android 2.3</rdfs:comment>
	</owl:Class>
	<owl:Class rdf:about="&android-2_3;AndroidSpeechTts">
		<owl:equivalentClass rdf:resource="&android-2_2;AndroidSpeechTts"/>
		<rdfs:subClassOf rdf:resource="&java;JavaAPIPart"/>
		<rdfs:seeAlso rdf:resource="&android-2_3;AndroidContent"/>
		<rdfs:seeAlso rdf:resource="&android-2_3;JavaUtil"/>
		<rdfs:seeAlso rdf:resource="&android-2_3;JavaLang"/>
		<rdfs:comment xml:lang="en">Java API part implementing the android.speech.tts package for Android 2.3</rdfs:comment>
	</owl:Class>
	<owl:Class rdf:about="&android-2_3;JavaxXmlAPI">
		<owl:equivalentClass rdf:resource="&java-se-6;JavaxXmlAPI"/>
		<owl:equivalentClass rdf:resource="&android-2_2;JavaxXmlAPI"/>
		<rdfs:subClassOf rdf:resource="&java;JavaAPI"/>
		<rdfs:comment xml:lang="en">JavaLibrary implementing the javax.xml package for Android 2.3</rdfs:comment>
		<rdfs:comment xml:lang="OWLManchester">platform:comprisesInterfacePart some JavaxXml</rdfs:comment>
	</owl:Class>
	<owl:Class rdf:about="&android-2_3;JavaxXmlDatatypeAPI">
		<owl:equivalentClass rdf:resource="&java-se-6;JavaxXmlDatatypeAPI"/>
		<rdfs:subClassOf rdf:resource="&android-2_2;JavaxXmlDatatypeAPI"/>
		<rdfs:comment xml:lang="en">JavaLibrary implementing the javax.xml.datatype package for Android 2.3</rdfs:comment>
		<rdfs:comment xml:lang="OWLManchester">platform:comprisesInterfacePart some JavaxXmlDatatype</rdfs:comment>
	</owl:Class>
	<owl:Class rdf:about="&android-2_3;JavaxXmlNamespaceAPI">
		<owl:equivalentClass rdf:resource="&java-se-6;JavaxXmlNamespaceAPI"/>
		<owl:equivalentClass rdf:resource="&android-2_2;JavaxXmlNamespaceAPI"/>
		<rdfs:subClassOf rdf:resource="&java;JavaAPI"/>
		<rdfs:comment xml:lang="en">JavaLibrary implementing the javax.xml.namespace package for Android 2.3</rdfs:comment>
		<rdfs:comment xml:lang="OWLManchester">platform:comprisesInterfacePart some JavaxXmlNamespace</rdfs:comment>
	</owl:Class>
	<owl:Class rdf:about="&android-2_3;JavaxXmlXpathAPI">
		<owl:equivalentClass rdf:resource="&java-se-6;JavaxXmlXpathAPI"/>
		<owl:equivalentClass rdf:resource="&android-2_2;JavaxXmlXpathAPI"/>
		<rdfs:subClassOf rdf:resource="&java;JavaAPI"/>
		<rdfs:comment xml:lang="en">JavaLibrary implementing the javax.xml.xpath package for Android 2.3</rdfs:comment>
		<rdfs:comment xml:lang="OWLManchester">platform:comprisesInterfacePart some JavaxXmlXpath</rdfs:comment>
	</owl:Class>
	<owl:Class rdf:about="&android-2_3;JavaxXmlTransformAPI">
		<owl:equivalentClass rdf:resource="&java-se-6;JavaxXmlTransformAPI"/>
		<rdfs:subClassOf rdf:resource="&android-2_2;JavaxXmlTransformAPI"/>
		<rdfs:comment xml:lang="en">JavaLibrary implementing the javax.xml.transform package for Android 2.3</rdfs:comment>
		<rdfs:comment xml:lang="OWLManchester">platform:comprisesInterfacePart some JavaxXmlTransform</rdfs:comment>
	</owl:Class>
	<owl:Class rdf:about="&android-2_3;JavaxXmlTransformDomAPI">
		<owl:equivalentClass rdf:resource="&java-se-6;JavaxXmlTransformDomAPI"/>
		<owl:equivalentClass rdf:resource="&android-2_2;JavaxXmlTransformDomAPI"/>
		<rdfs:subClassOf rdf:resource="&java;JavaAPI"/>
		<rdfs:comment xml:lang="en">JavaLibrary implementing the javax.xml.transform.dom package for Android 2.3</rdfs:comment>
		<rdfs:comment xml:lang="OWLManchester">platform:comprisesInterfacePart some JavaxXmlTransformDom</rdfs:comment>
	</owl:Class>
	<owl:Class rdf:about="&android-2_3;JavaxXmlTransformSaxAPI">
		<owl:equivalentClass rdf:resource="&java-se-6;JavaxXmlTransformSaxAPI"/>
		<rdfs:subClassOf rdf:resource="&android-2_2;JavaxXmlTransformSaxAPI"/>
		<rdfs:comment xml:lang="en">JavaLibrary implementing the javax.xml.transform.sax package for Android 2.3</rdfs:comment>
		<rdfs:comment xml:lang="OWLManchester">platform:comprisesInterfacePart some JavaxXmlTransformSax</rdfs:comment>
	</owl:Class>
	<owl:Class rdf:about="&android-2_3;JavaxXmlTransformStreamAPI">
		<owl:equivalentClass rdf:resource="&java-se-6;JavaxXmlTransformStreamAPI"/>
		<owl:equivalentClass rdf:resource="&android-2_2;JavaxXmlTransformStreamAPI"/>
		<rdfs:subClassOf rdf:resource="&java;JavaAPI"/>
		<rdfs:comment xml:lang="en">JavaLibrary implementing the javax.xml.transform.stream package for Android 2.3</rdfs:comment>
		<rdfs:comment xml:lang="OWLManchester">platform:comprisesInterfacePart some JavaxXmlTransformStream</rdfs:comment>
	</owl:Class>
	<owl:Class rdf:about="&android-2_3;JavaxXmlParsersAPI">
		<owl:equivalentClass rdf:resource="&java-se-6;JavaxXmlParsersAPI"/>
		<rdfs:subClassOf rdf:resource="&android-2_2;JavaxXmlParsersAPI"/>
		<rdfs:comment xml:lang="en">JavaLibrary implementing the javax.xml.parsers package for Android 2.3</rdfs:comment>
		<rdfs:comment xml:lang="OWLManchester">platform:comprisesInterfacePart some JavaxXmlParsers</rdfs:comment>
	</owl:Class>
	<owl:Class rdf:about="&android-2_3;JavaxXmlValidationAPI">
		<rdfs:subClassOf rdf:resource="&java-se-6;JavaxXmlValidationAPI"/>
		<rdfs:subClassOf rdf:resource="&android-2_2;JavaxXmlValidationAPI"/>
		<rdfs:comment xml:lang="en">JavaLibrary implementing the javax.xml.validation package for Android 2.3</rdfs:comment>
		<rdfs:comment xml:lang="OWLManchester">platform:comprisesInterfacePart some JavaxXmlValidation</rdfs:comment>
	</owl:Class>
	<owl:Class rdf:about="&android-2_3;JavaxSecurityCertAPI">
		<owl:equivalentClass rdf:resource="&java-se-6;JavaxSecurityCertAPI"/>
		<owl:equivalentClass rdf:resource="&android-2_2;JavaxSecurityCertAPI"/>
		<rdfs:subClassOf rdf:resource="&java;JavaAPI"/>
		<rdfs:comment xml:lang="en">JavaLibrary implementing the javax.security.cert package for Android 2.3</rdfs:comment>
		<rdfs:comment xml:lang="OWLManchester">platform:comprisesInterfacePart some JavaxSecurityCert</rdfs:comment>
	</owl:Class>
	<owl:Class rdf:about="&android-2_3;JavaxSecurityAuthAPI">
		<owl:equivalentClass rdf:resource="&android-2_2;JavaxSecurityAuthAPI"/>
		<rdfs:subClassOf rdf:resource="&java;JavaAPI"/>
		<rdfs:comment xml:lang="en">JavaLibrary implementing the javax.security.auth package for Android 2.3</rdfs:comment>
		<rdfs:comment xml:lang="OWLManchester">platform:comprisesInterfacePart some JavaxSecurityAuth</rdfs:comment>
	</owl:Class>
	<owl:Class rdf:about="&android-2_3;JavaxSecurityAuthCallbackAPI">
		<owl:equivalentClass rdf:resource="&android-2_2;JavaxSecurityAuthCallbackAPI"/>
		<rdfs:subClassOf rdf:resource="&java;JavaAPI"/>
		<rdfs:comment xml:lang="en">JavaLibrary implementing the javax.security.auth.callback package for Android 2.3</rdfs:comment>
		<rdfs:comment xml:lang="OWLManchester">platform:comprisesInterfacePart some JavaxSecurityAuthCallback</rdfs:comment>
	</owl:Class>
	<owl:Class rdf:about="&android-2_3;JavaxSecurityAuthLoginAPI">
		<owl:equivalentClass rdf:resource="&android-2_2;JavaxSecurityAuthLoginAPI"/>
		<rdfs:subClassOf rdf:resource="&java;JavaAPI"/>
		<rdfs:comment xml:lang="en">JavaLibrary implementing the javax.security.auth.login package for Android 2.3</rdfs:comment>
		<rdfs:comment xml:lang="OWLManchester">platform:comprisesInterfacePart some JavaxSecurityAuthLogin</rdfs:comment>
	</owl:Class>
	<owl:Class rdf:about="&android-2_3;JavaxSecurityAuthX500API">
		<rdfs:subClassOf rdf:resource="&android-2_2;JavaxSecurityAuthX500API"/>
		<rdfs:comment xml:lang="en">JavaLibrary implementing the javax.security.auth.x500 package for Android 2.3</rdfs:comment>
		<rdfs:comment xml:lang="OWLManchester">platform:comprisesInterfacePart some JavaxSecurityAuthX500</rdfs:comment>
	</owl:Class>
	<owl:Class rdf:about="&android-2_3;JavaxSqlAPI">
		<rdfs:subClassOf rdf:resource="&android-2_2;JavaxSqlAPI"/>
		<rdfs:comment xml:lang="en">JavaLibrary implementing the javax.sql package for Android 2.3</rdfs:comment>
		<rdfs:comment xml:lang="OWLManchester">platform:comprisesInterfacePart some JavaxSql</rdfs:comment>
	</owl:Class>
	<owl:Class rdf:about="&android-2_3;JavaxCryptoAPI">
		<owl:equivalentClass rdf:resource="&java-se-6;JavaxCryptoAPI"/>
		<owl:equivalentClass rdf:resource="&android-2_2;JavaxCryptoAPI"/>
		<rdfs:subClassOf rdf:resource="&java;JavaAPI"/>
		<rdfs:comment xml:lang="en">JavaLibrary implementing the javax.crypto package for Android 2.3</rdfs:comment>
		<rdfs:comment xml:lang="OWLManchester">platform:comprisesInterfacePart some JavaxCrypto</rdfs:comment>
	</owl:Class>
	<owl:Class rdf:about="&android-2_3;JavaxCryptoInterfacesAPI">
		<owl:equivalentClass rdf:resource="&java-se-6;JavaxCryptoInterfacesAPI"/>
		<owl:equivalentClass rdf:resource="&android-2_2;JavaxCryptoInterfacesAPI"/>
		<rdfs:subClassOf rdf:resource="&java;JavaAPI"/>
		<rdfs:comment xml:lang="en">JavaLibrary implementing the javax.crypto.interfaces package for Android 2.3</rdfs:comment>
		<rdfs:comment xml:lang="OWLManchester">platform:comprisesInterfacePart some JavaxCryptoInterfaces</rdfs:comment>
	</owl:Class>
	<owl:Class rdf:about="&android-2_3;JavaxCryptoSpecAPI">
		<owl:equivalentClass rdf:resource="&java-se-6;JavaxCryptoSpecAPI"/>
		<owl:equivalentClass rdf:resource="&android-2_2;JavaxCryptoSpecAPI"/>
		<rdfs:subClassOf rdf:resource="&java;JavaAPI"/>
		<rdfs:comment xml:lang="en">JavaLibrary implementing the javax.crypto.spec package for Android 2.3</rdfs:comment>
		<rdfs:comment xml:lang="OWLManchester">platform:comprisesInterfacePart some JavaxCryptoSpec</rdfs:comment>
	</owl:Class>
	<owl:Class rdf:about="&android-2_3;JavaxMicroeditionKhronosEglAPI">
		<owl:equivalentClass rdf:resource="&android-2_2;JavaxMicroeditionKhronosEglAPI"/>
		<rdfs:subClassOf rdf:resource="&java;JavaAPI"/>
		<rdfs:comment xml:lang="en">JavaLibrary implementing the javax.microedition.khronos.egl package for Android 2.3</rdfs:comment>
		<rdfs:comment xml:lang="OWLManchester">platform:comprisesInterfacePart some JavaxMicroeditionKhronosEgl</rdfs:comment>
	</owl:Class>
	<owl:Class rdf:about="&android-2_3;JavaxMicroeditionKhronosOpenglesAPI">
		<owl:equivalentClass rdf:resource="&android-2_2;JavaxMicroeditionKhronosOpenglesAPI"/>
		<rdfs:subClassOf rdf:resource="&java;JavaAPI"/>
		<rdfs:comment xml:lang="en">JavaLibrary implementing the javax.microedition.khronos.opengles package for Android 2.3</rdfs:comment>
		<rdfs:comment xml:lang="OWLManchester">platform:comprisesInterfacePart some JavaxMicroeditionKhronosOpengles</rdfs:comment>
	</owl:Class>
	<owl:Class rdf:about="&android-2_3;JavaxNetAPI">
		<owl:equivalentClass rdf:resource="&java-se-6;JavaxNetAPI"/>
		<owl:equivalentClass rdf:resource="&android-2_2;JavaxNetAPI"/>
		<rdfs:subClassOf rdf:resource="&java;JavaAPI"/>
		<rdfs:comment xml:lang="en">JavaLibrary implementing the javax.net package for Android 2.3</rdfs:comment>
		<rdfs:comment xml:lang="OWLManchester">platform:comprisesInterfacePart some JavaxNet</rdfs:comment>
	</owl:Class>
	<owl:Class rdf:about="&android-2_3;JavaxNetSslAPI">
		<owl:equivalentClass rdf:resource="&java-se-6;JavaxNetSslAPI"/>
		<rdfs:subClassOf rdf:resource="&android-2_2;JavaxNetSslAPI"/>
		<rdfs:comment xml:lang="en">JavaLibrary implementing the javax.net.ssl package for Android 2.3</rdfs:comment>
		<rdfs:comment xml:lang="OWLManchester">platform:comprisesInterfacePart some JavaxNetSsl</rdfs:comment>
	</owl:Class>
	<owl:Class rdf:about="&android-2_3;JavaLangAPI">
		<rdfs:subClassOf rdf:resource="&java;JavaAPI"/>
		<rdfs:comment xml:lang="en">JavaLibrary implementing the java.lang package for Android 2.3</rdfs:comment>
		<rdfs:comment xml:lang="OWLManchester">platform:comprisesInterfacePart some JavaLang</rdfs:comment>
	</owl:Class>
	<owl:Class rdf:about="&android-2_3;JavaLangReflectAPI">
		<owl:equivalentClass rdf:resource="&java-se-6;JavaLangReflectAPI"/>
		<owl:equivalentClass rdf:resource="&android-2_2;JavaLangReflectAPI"/>
		<rdfs:subClassOf rdf:resource="&java;JavaAPI"/>
		<rdfs:comment xml:lang="en">JavaLibrary implementing the java.lang.reflect package for Android 2.3</rdfs:comment>
		<rdfs:comment xml:lang="OWLManchester">platform:comprisesInterfacePart some JavaLangReflect</rdfs:comment>
	</owl:Class>
	<owl:Class rdf:about="&android-2_3;JavaLangAnnotationAPI">
		<owl:equivalentClass rdf:resource="&java-se-6;JavaLangAnnotationAPI"/>
		<rdfs:subClassOf rdf:resource="&android-2_2;JavaLangAnnotationAPI"/>
		<rdfs:comment xml:lang="en">JavaLibrary implementing the java.lang.annotation package for Android 2.3</rdfs:comment>
		<rdfs:comment xml:lang="OWLManchester">platform:comprisesInterfacePart some JavaLangAnnotation</rdfs:comment>
	</owl:Class>
	<owl:Class rdf:about="&android-2_3;JavaLangRefAPI">
		<owl:equivalentClass rdf:resource="&java-se-6;JavaLangRefAPI"/>
		<owl:equivalentClass rdf:resource="&android-2_2;JavaLangRefAPI"/>
		<rdfs:subClassOf rdf:resource="&java;JavaAPI"/>
		<rdfs:comment xml:lang="en">JavaLibrary implementing the java.lang.ref package for Android 2.3</rdfs:comment>
		<rdfs:comment xml:lang="OWLManchester">platform:comprisesInterfacePart some JavaLangRef</rdfs:comment>
	</owl:Class>
	<owl:Class rdf:about="&android-2_3;JavaUtilAPI">
		<owl:equivalentClass rdf:resource="&java-se-6;JavaUtilAPI"/>
		<rdfs:subClassOf rdf:resource="&android-2_2;JavaUtilAPI"/>
		<rdfs:comment xml:lang="en">JavaLibrary implementing the java.util package for Android 2.3</rdfs:comment>
		<rdfs:comment xml:lang="OWLManchester">platform:comprisesInterfacePart some JavaUtil</rdfs:comment>
	</owl:Class>
	<owl:Class rdf:about="&android-2_3;JavaUtilJarAPI">
		<owl:equivalentClass rdf:resource="&java-se-6;JavaUtilJarAPI"/>
		<owl:equivalentClass rdf:resource="&android-2_2;JavaUtilJarAPI"/>
		<rdfs:subClassOf rdf:resource="&java;JavaAPI"/>
		<rdfs:comment xml:lang="en">JavaLibrary implementing the java.util.jar package for Android 2.3</rdfs:comment>
		<rdfs:comment xml:lang="OWLManchester">platform:comprisesInterfacePart some JavaUtilJar</rdfs:comment>
	</owl:Class>
	<owl:Class rdf:about="&android-2_3;JavaUtilZipAPI">
		<owl:equivalentClass rdf:resource="&java-se-6;JavaUtilZipAPI"/>
		<rdfs:subClassOf rdf:resource="&android-2_2;JavaUtilZipAPI"/>
		<rdfs:comment xml:lang="en">JavaLibrary implementing the java.util.zip package for Android 2.3</rdfs:comment>
		<rdfs:comment xml:lang="OWLManchester">platform:comprisesInterfacePart some JavaUtilZip</rdfs:comment>
	</owl:Class>
	<owl:Class rdf:about="&android-2_3;JavaUtilPrefsAPI">
		<owl:equivalentClass rdf:resource="&java-se-6;JavaUtilPrefsAPI"/>
		<owl:equivalentClass rdf:resource="&android-2_2;JavaUtilPrefsAPI"/>
		<rdfs:subClassOf rdf:resource="&java;JavaAPI"/>
		<rdfs:comment xml:lang="en">JavaLibrary implementing the java.util.prefs package for Android 2.3</rdfs:comment>
		<rdfs:comment xml:lang="OWLManchester">platform:comprisesInterfacePart some JavaUtilPrefs</rdfs:comment>
	</owl:Class>
	<owl:Class rdf:about="&android-2_3;JavaUtilRegexAPI">
		<owl:equivalentClass rdf:resource="&java-se-6;JavaUtilRegexAPI"/>
		<owl:equivalentClass rdf:resource="&android-2_2;JavaUtilRegexAPI"/>
		<rdfs:subClassOf rdf:resource="&java;JavaAPI"/>
		<rdfs:comment xml:lang="en">JavaLibrary implementing the java.util.regex package for Android 2.3</rdfs:comment>
		<rdfs:comment xml:lang="OWLManchester">platform:comprisesInterfacePart some JavaUtilRegex</rdfs:comment>
	</owl:Class>
	<owl:Class rdf:about="&android-2_3;JavaUtilConcurrentAPI">
		<rdfs:subClassOf rdf:resource="&android-2_2;JavaUtilConcurrentAPI"/>
		<rdfs:comment xml:lang="en">JavaLibrary implementing the java.util.concurrent package for Android 2.3</rdfs:comment>
		<rdfs:comment xml:lang="OWLManchester">platform:comprisesInterfacePart some JavaUtilConcurrent</rdfs:comment>
	</owl:Class>
	<owl:Class rdf:about="&android-2_3;JavaUtilConcurrentAtomicAPI">
		<owl:equivalentClass rdf:resource="&java-se-6;JavaUtilConcurrentAtomicAPI"/>
		<rdfs:subClassOf rdf:resource="&android-2_2;JavaUtilConcurrentAtomicAPI"/>
		<rdfs:comment xml:lang="en">JavaLibrary implementing the java.util.concurrent.atomic package for Android 2.3</rdfs:comment>
		<rdfs:comment xml:lang="OWLManchester">platform:comprisesInterfacePart some JavaUtilConcurrentAtomic</rdfs:comment>
	</owl:Class>
	<owl:Class rdf:about="&android-2_3;JavaUtilConcurrentLocksAPI">
		<owl:equivalentClass rdf:resource="&java-se-6;JavaUtilConcurrentLocksAPI"/>
		<rdfs:subClassOf rdf:resource="&android-2_2;JavaUtilConcurrentLocksAPI"/>
		<rdfs:comment xml:lang="en">JavaLibrary implementing the java.util.concurrent.locks package for Android 2.3</rdfs:comment>
		<rdfs:comment xml:lang="OWLManchester">platform:comprisesInterfacePart some JavaUtilConcurrentLocks</rdfs:comment>
	</owl:Class>
	<owl:Class rdf:about="&android-2_3;JavaUtilLoggingAPI">
		<owl:equivalentClass rdf:resource="&java-se-6;JavaUtilLoggingAPI"/>
		<rdfs:subClassOf rdf:resource="&android-2_2;JavaUtilLoggingAPI"/>
		<rdfs:comment xml:lang="en">JavaLibrary implementing the java.util.logging package for Android 2.3</rdfs:comment>
		<rdfs:comment xml:lang="OWLManchester">platform:comprisesInterfacePart some JavaUtilLogging</rdfs:comment>
	</owl:Class>
	<owl:Class rdf:about="&android-2_3;JavaMathAPI">
		<owl:equivalentClass rdf:resource="&java-se-6;JavaMathAPI"/>
		<rdfs:subClassOf rdf:resource="&android-2_2;JavaMathAPI"/>
		<rdfs:comment xml:lang="en">JavaLibrary implementing the java.math package for Android 2.3</rdfs:comment>
		<rdfs:comment xml:lang="OWLManchester">platform:comprisesInterfacePart some JavaMath</rdfs:comment>
	</owl:Class>
	<owl:Class rdf:about="&android-2_3;JavaIoAPI">
		<owl:equivalentClass rdf:resource="&java-se-6;JavaIoAPI"/>
		<rdfs:subClassOf rdf:resource="&android-2_2;JavaIoAPI"/>
		<rdfs:comment xml:lang="en">JavaLibrary implementing the java.io package for Android 2.3</rdfs:comment>
		<rdfs:comment xml:lang="OWLManchester">platform:comprisesInterfacePart some JavaIo</rdfs:comment>
	</owl:Class>
	<owl:Class rdf:about="&android-2_3;JavaNetAPI">
		<owl:equivalentClass rdf:resource="&java-se-6;JavaNetAPI"/>
		<rdfs:subClassOf rdf:resource="&android-2_2;JavaNetAPI"/>
		<rdfs:comment xml:lang="en">JavaLibrary implementing the java.net package for Android 2.3</rdfs:comment>
		<rdfs:comment xml:lang="OWLManchester">platform:comprisesInterfacePart some JavaNet</rdfs:comment>
	</owl:Class>
	<owl:Class rdf:about="&android-2_3;JavaSecurityAPI">
		<rdfs:subClassOf rdf:resource="&android-2_2;JavaSecurityAPI"/>
		<rdfs:comment xml:lang="en">JavaLibrary implementing the java.security package for Android 2.3</rdfs:comment>
		<rdfs:comment xml:lang="OWLManchester">platform:comprisesInterfacePart some JavaSecurity</rdfs:comment>
	</owl:Class>
	<owl:Class rdf:about="&android-2_3;JavaSecuritySpecAPI">
		<owl:equivalentClass rdf:resource="&java-se-6;JavaSecuritySpecAPI"/>
		<owl:equivalentClass rdf:resource="&android-2_2;JavaSecuritySpecAPI"/>
		<rdfs:subClassOf rdf:resource="&java;JavaAPI"/>
		<rdfs:comment xml:lang="en">JavaLibrary implementing the java.security.spec package for Android 2.3</rdfs:comment>
		<rdfs:comment xml:lang="OWLManchester">platform:comprisesInterfacePart some JavaSecuritySpec</rdfs:comment>
	</owl:Class>
	<owl:Class rdf:about="&android-2_3;JavaSecurityCertAPI">
		<owl:equivalentClass rdf:resource="&java-se-6;JavaSecurityCertAPI"/>
		<owl:equivalentClass rdf:resource="&android-2_2;JavaSecurityCertAPI"/>
		<rdfs:subClassOf rdf:resource="&java;JavaAPI"/>
		<rdfs:comment xml:lang="en">JavaLibrary implementing the java.security.cert package for Android 2.3</rdfs:comment>
		<rdfs:comment xml:lang="OWLManchester">platform:comprisesInterfacePart some JavaSecurityCert</rdfs:comment>
	</owl:Class>
	<owl:Class rdf:about="&android-2_3;JavaSecurityInterfacesAPI">
		<owl:equivalentClass rdf:resource="&java-se-6;JavaSecurityInterfacesAPI"/>
		<owl:equivalentClass rdf:resource="&android-2_2;JavaSecurityInterfacesAPI"/>
		<rdfs:subClassOf rdf:resource="&java;JavaAPI"/>
		<rdfs:comment xml:lang="en">JavaLibrary implementing the java.security.interfaces package for Android 2.3</rdfs:comment>
		<rdfs:comment xml:lang="OWLManchester">platform:comprisesInterfacePart some JavaSecurityInterfaces</rdfs:comment>
	</owl:Class>
	<owl:Class rdf:about="&android-2_3;JavaSecurityAclAPI">
		<owl:equivalentClass rdf:resource="&java-se-6;JavaSecurityAclAPI"/>
		<owl:equivalentClass rdf:resource="&android-2_2;JavaSecurityAclAPI"/>
		<rdfs:subClassOf rdf:resource="&java;JavaAPI"/>
		<rdfs:comment xml:lang="en">JavaLibrary implementing the java.security.acl package for Android 2.3</rdfs:comment>
		<rdfs:comment xml:lang="OWLManchester">platform:comprisesInterfacePart some JavaSecurityAcl</rdfs:comment>
	</owl:Class>
	<owl:Class rdf:about="&android-2_3;JavaSqlAPI">
		<owl:equivalentClass rdf:resource="&java-se-6;JavaSqlAPI"/>
		<rdfs:subClassOf rdf:resource="&android-2_2;JavaSqlAPI"/>
		<rdfs:comment xml:lang="en">JavaLibrary implementing the java.sql package for Android 2.3</rdfs:comment>
		<rdfs:comment xml:lang="OWLManchester">platform:comprisesInterfacePart some JavaSql</rdfs:comment>
	</owl:Class>
	<owl:Class rdf:about="&android-2_3;JavaNioAPI">
		<owl:equivalentClass rdf:resource="&java-se-6;JavaNioAPI"/>
		<rdfs:subClassOf rdf:resource="&android-2_2;JavaNioAPI"/>
		<rdfs:comment xml:lang="en">JavaLibrary implementing the java.nio package for Android 2.3</rdfs:comment>
		<rdfs:comment xml:lang="OWLManchester">platform:comprisesInterfacePart some JavaNio</rdfs:comment>
	</owl:Class>
	<owl:Class rdf:about="&android-2_3;JavaNioChannelsAPI">
		<owl:equivalentClass rdf:resource="&java-se-6;JavaNioChannelsAPI"/>
		<owl:equivalentClass rdf:resource="&android-2_2;JavaNioChannelsAPI"/>
		<rdfs:subClassOf rdf:resource="&java;JavaAPI"/>
		<rdfs:comment xml:lang="en">JavaLibrary implementing the java.nio.channels package for Android 2.3</rdfs:comment>
		<rdfs:comment xml:lang="OWLManchester">platform:comprisesInterfacePart some JavaNioChannels</rdfs:comment>
	</owl:Class>
	<owl:Class rdf:about="&android-2_3;JavaNioChannelsSpiAPI">
		<owl:equivalentClass rdf:resource="&java-se-6;JavaNioChannelsSpiAPI"/>
		<owl:equivalentClass rdf:resource="&android-2_2;JavaNioChannelsSpiAPI"/>
		<rdfs:subClassOf rdf:resource="&java;JavaAPI"/>
		<rdfs:comment xml:lang="en">JavaLibrary implementing the java.nio.channels.spi package for Android 2.3</rdfs:comment>
		<rdfs:comment xml:lang="OWLManchester">platform:comprisesInterfacePart some JavaNioChannelsSpi</rdfs:comment>
	</owl:Class>
	<owl:Class rdf:about="&android-2_3;JavaNioCharsetAPI">
		<owl:equivalentClass rdf:resource="&java-se-6;JavaNioCharsetAPI"/>
		<owl:equivalentClass rdf:resource="&android-2_2;JavaNioCharsetAPI"/>
		<rdfs:subClassOf rdf:resource="&java;JavaAPI"/>
		<rdfs:comment xml:lang="en">JavaLibrary implementing the java.nio.charset package for Android 2.3</rdfs:comment>
		<rdfs:comment xml:lang="OWLManchester">platform:comprisesInterfacePart some JavaNioCharset</rdfs:comment>
	</owl:Class>
	<owl:Class rdf:about="&android-2_3;JavaNioCharsetSpiAPI">
		<owl:equivalentClass rdf:resource="&java-se-6;JavaNioCharsetSpiAPI"/>
		<owl:equivalentClass rdf:resource="&android-2_2;JavaNioCharsetSpiAPI"/>
		<rdfs:subClassOf rdf:resource="&java;JavaAPI"/>
		<rdfs:comment xml:lang="en">JavaLibrary implementing the java.nio.charset.spi package for Android 2.3</rdfs:comment>
		<rdfs:comment xml:lang="OWLManchester">platform:comprisesInterfacePart some JavaNioCharsetSpi</rdfs:comment>
	</owl:Class>
	<owl:Class rdf:about="&android-2_3;JavaBeansAPI">
		<owl:equivalentClass rdf:resource="&android-2_2;JavaBeansAPI"/>
		<rdfs:subClassOf rdf:resource="&java;JavaAPI"/>
		<rdfs:comment xml:lang="en">JavaLibrary implementing the java.beans package for Android 2.3</rdfs:comment>
		<rdfs:comment xml:lang="OWLManchester">platform:comprisesInterfacePart some JavaBeans</rdfs:comment>
	</owl:Class>
	<owl:Class rdf:about="&android-2_3;JavaTextAPI">
		<rdfs:subClassOf rdf:resource="&java-se-6;JavaTextAPI"/>
		<rdfs:comment xml:lang="en">JavaLibrary implementing the java.text package for Android 2.3</rdfs:comment>
		<rdfs:comment xml:lang="OWLManchester">platform:comprisesInterfacePart some JavaText</rdfs:comment>
	</owl:Class>
	<owl:Class rdf:about="&android-2_3;JavaAwtFontAPI">
		<rdfs:subClassOf rdf:resource="&android-2_2;JavaAwtFontAPI"/>
		<rdfs:comment xml:lang="en">JavaLibrary implementing the java.awt.font package for Android 2.3</rdfs:comment>
		<rdfs:comment xml:lang="OWLManchester">platform:comprisesInterfacePart some JavaAwtFont</rdfs:comment>
	</owl:Class>
	<owl:Class rdf:about="&android-2_3;OrgXmlSaxAPI">
		<owl:equivalentClass rdf:resource="&java-se-6;OrgXmlSaxAPI"/>
		<owl:equivalentClass rdf:resource="&android-2_2;OrgXmlSaxAPI"/>
		<rdfs:subClassOf rdf:resource="&java;JavaAPI"/>
		<rdfs:comment xml:lang="en">JavaLibrary implementing the org.xml.sax package for Android 2.3</rdfs:comment>
		<rdfs:comment xml:lang="OWLManchester">platform:comprisesInterfacePart some OrgXmlSax</rdfs:comment>
	</owl:Class>
	<owl:Class rdf:about="&android-2_3;OrgXmlSaxExtAPI">
		<owl:equivalentClass rdf:resource="&java-se-6;OrgXmlSaxExtAPI"/>
		<owl:equivalentClass rdf:resource="&android-2_2;OrgXmlSaxExtAPI"/>
		<rdfs:subClassOf rdf:resource="&java;JavaAPI"/>
		<rdfs:comment xml:lang="en">JavaLibrary implementing the org.xml.sax.ext package for Android 2.3</rdfs:comment>
		<rdfs:comment xml:lang="OWLManchester">platform:comprisesInterfacePart some OrgXmlSaxExt</rdfs:comment>
	</owl:Class>
	<owl:Class rdf:about="&android-2_3;OrgXmlSaxHelpersAPI">
		<owl:equivalentClass rdf:resource="&java-se-6;OrgXmlSaxHelpersAPI"/>
		<owl:equivalentClass rdf:resource="&android-2_2;OrgXmlSaxHelpersAPI"/>
		<rdfs:subClassOf rdf:resource="&java;JavaAPI"/>
		<rdfs:comment xml:lang="en">JavaLibrary implementing the org.xml.sax.helpers package for Android 2.3</rdfs:comment>
		<rdfs:comment xml:lang="OWLManchester">platform:comprisesInterfacePart some OrgXmlSaxHelpers</rdfs:comment>
	</owl:Class>
	<owl:Class rdf:about="&android-2_3;OrgW3cDomAPI">
		<owl:equivalentClass rdf:resource="&java-se-6;OrgW3cDomAPI"/>
		<owl:equivalentClass rdf:resource="&android-2_2;OrgW3cDomAPI"/>
		<rdfs:subClassOf rdf:resource="&java;JavaAPI"/>
		<rdfs:comment xml:lang="en">JavaLibrary implementing the org.w3c.dom package for Android 2.3</rdfs:comment>
		<rdfs:comment xml:lang="OWLManchester">platform:comprisesInterfacePart some OrgW3cDom</rdfs:comment>
	</owl:Class>
	<owl:Class rdf:about="&android-2_3;OrgW3cDomLsAPI">
		<owl:equivalentClass rdf:resource="&android-2_2;OrgW3cDomLsAPI"/>
		<rdfs:subClassOf rdf:resource="&java;JavaAPI"/>
		<rdfs:comment xml:lang="en">JavaLibrary implementing the org.w3c.dom.ls package for Android 2.3</rdfs:comment>
		<rdfs:comment xml:lang="OWLManchester">platform:comprisesInterfacePart some OrgW3cDomLs</rdfs:comment>
	</owl:Class>
	<owl:Class rdf:about="&android-2_3;OrgXmlpullV1API">
		<owl:equivalentClass rdf:resource="&android-2_2;OrgXmlpullV1API"/>
		<rdfs:subClassOf rdf:resource="&java;JavaAPI"/>
		<rdfs:comment xml:lang="en">JavaLibrary implementing the org.xmlpull.v1 package for Android 2.3</rdfs:comment>
		<rdfs:comment xml:lang="OWLManchester">platform:comprisesInterfacePart some OrgXmlpullV1</rdfs:comment>
	</owl:Class>
	<owl:Class rdf:about="&android-2_3;OrgXmlpullV1Sax2API">
		<owl:equivalentClass rdf:resource="&android-2_2;OrgXmlpullV1Sax2API"/>
		<rdfs:subClassOf rdf:resource="&java;JavaAPI"/>
		<rdfs:comment xml:lang="en">JavaLibrary implementing the org.xmlpull.v1.sax2 package for Android 2.3</rdfs:comment>
		<rdfs:comment xml:lang="OWLManchester">platform:comprisesInterfacePart some OrgXmlpullV1Sax2</rdfs:comment>
	</owl:Class>
	<owl:Class rdf:about="&android-2_3;OrgApacheHttpAPI">
		<owl:equivalentClass rdf:resource="&android-2_2;OrgApacheHttpAPI"/>
		<rdfs:subClassOf rdf:resource="&java;JavaAPI"/>
		<rdfs:comment xml:lang="en">JavaLibrary implementing the org.apache.http package for Android 2.3</rdfs:comment>
		<rdfs:comment xml:lang="OWLManchester">platform:comprisesInterfacePart some OrgApacheHttp</rdfs:comment>
	</owl:Class>
	<owl:Class rdf:about="&android-2_3;OrgApacheHttpClientAPI">
		<owl:equivalentClass rdf:resource="&android-2_2;OrgApacheHttpClientAPI"/>
		<rdfs:subClassOf rdf:resource="&java;JavaAPI"/>
		<rdfs:comment xml:lang="en">JavaLibrary implementing the org.apache.http.client package for Android 2.3</rdfs:comment>
		<rdfs:comment xml:lang="OWLManchester">platform:comprisesInterfacePart some OrgApacheHttpClient</rdfs:comment>
	</owl:Class>
	<owl:Class rdf:about="&android-2_3;OrgApacheHttpClientMethodsAPI">
		<owl:equivalentClass rdf:resource="&android-2_2;OrgApacheHttpClientMethodsAPI"/>
		<rdfs:subClassOf rdf:resource="&java;JavaAPI"/>
		<rdfs:comment xml:lang="en">JavaLibrary implementing the org.apache.http.client.methods package for Android 2.3</rdfs:comment>
		<rdfs:comment xml:lang="OWLManchester">platform:comprisesInterfacePart some OrgApacheHttpClientMethods</rdfs:comment>
	</owl:Class>
	<owl:Class rdf:about="&android-2_3;OrgApacheHttpClientEntityAPI">
		<owl:equivalentClass rdf:resource="&android-2_2;OrgApacheHttpClientEntityAPI"/>
		<rdfs:subClassOf rdf:resource="&java;JavaAPI"/>
		<rdfs:comment xml:lang="en">JavaLibrary implementing the org.apache.http.client.entity package for Android 2.3</rdfs:comment>
		<rdfs:comment xml:lang="OWLManchester">platform:comprisesInterfacePart some OrgApacheHttpClientEntity</rdfs:comment>
	</owl:Class>
	<owl:Class rdf:about="&android-2_3;OrgApacheHttpClientParamsAPI">
		<owl:equivalentClass rdf:resource="&android-2_2;OrgApacheHttpClientParamsAPI"/>
		<rdfs:subClassOf rdf:resource="&java;JavaAPI"/>
		<rdfs:comment xml:lang="en">JavaLibrary implementing the org.apache.http.client.params package for Android 2.3</rdfs:comment>
		<rdfs:comment xml:lang="OWLManchester">platform:comprisesInterfacePart some OrgApacheHttpClientParams</rdfs:comment>
	</owl:Class>
	<owl:Class rdf:about="&android-2_3;OrgApacheHttpClientProtocolAPI">
		<owl:equivalentClass rdf:resource="&android-2_2;OrgApacheHttpClientProtocolAPI"/>
		<rdfs:subClassOf rdf:resource="&java;JavaAPI"/>
		<rdfs:comment xml:lang="en">JavaLibrary implementing the org.apache.http.client.protocol package for Android 2.3</rdfs:comment>
		<rdfs:comment xml:lang="OWLManchester">platform:comprisesInterfacePart some OrgApacheHttpClientProtocol</rdfs:comment>
	</owl:Class>
	<owl:Class rdf:about="&android-2_3;OrgApacheHttpClientUtilsAPI">
		<owl:equivalentClass rdf:resource="&android-2_2;OrgApacheHttpClientUtilsAPI"/>
		<rdfs:subClassOf rdf:resource="&java;JavaAPI"/>
		<rdfs:comment xml:lang="en">JavaLibrary implementing the org.apache.http.client.utils package for Android 2.3</rdfs:comment>
		<rdfs:comment xml:lang="OWLManchester">platform:comprisesInterfacePart some OrgApacheHttpClientUtils</rdfs:comment>
	</owl:Class>
	<owl:Class rdf:about="&android-2_3;OrgApacheHttpParamsAPI">
		<owl:equivalentClass rdf:resource="&android-2_2;OrgApacheHttpParamsAPI"/>
		<rdfs:subClassOf rdf:resource="&java;JavaAPI"/>
		<rdfs:comment xml:lang="en">JavaLibrary implementing the org.apache.http.params package for Android 2.3</rdfs:comment>
		<rdfs:comment xml:lang="OWLManchester">platform:comprisesInterfacePart some OrgApacheHttpParams</rdfs:comment>
	</owl:Class>
	<owl:Class rdf:about="&android-2_3;OrgApacheHttpConnAPI">
		<owl:equivalentClass rdf:resource="&android-2_2;OrgApacheHttpConnAPI"/>
		<rdfs:subClassOf rdf:resource="&java;JavaAPI"/>
		<rdfs:comment xml:lang="en">JavaLibrary implementing the org.apache.http.conn package for Android 2.3</rdfs:comment>
		<rdfs:comment xml:lang="OWLManchester">platform:comprisesInterfacePart some OrgApacheHttpConn</rdfs:comment>
	</owl:Class>
	<owl:Class rdf:about="&android-2_3;OrgApacheHttpConnSslAPI">
		<owl:equivalentClass rdf:resource="&android-2_2;OrgApacheHttpConnSslAPI"/>
		<rdfs:subClassOf rdf:resource="&java;JavaAPI"/>
		<rdfs:comment xml:lang="en">JavaLibrary implementing the org.apache.http.conn.ssl package for Android 2.3</rdfs:comment>
		<rdfs:comment xml:lang="OWLManchester">platform:comprisesInterfacePart some OrgApacheHttpConnSsl</rdfs:comment>
	</owl:Class>
	<owl:Class rdf:about="&android-2_3;OrgApacheHttpConnRoutingAPI">
		<rdfs:subClassOf rdf:resource="&android-2_2;OrgApacheHttpConnRoutingAPI"/>
		<rdfs:comment xml:lang="en">JavaLibrary implementing the org.apache.http.conn.routing package for Android 2.3</rdfs:comment>
		<rdfs:comment xml:lang="OWLManchester">platform:comprisesInterfacePart some OrgApacheHttpConnRouting</rdfs:comment>
	</owl:Class>
	<owl:Class rdf:about="&android-2_3;OrgApacheHttpConnSchemeAPI">
		<owl:equivalentClass rdf:resource="&android-2_2;OrgApacheHttpConnSchemeAPI"/>
		<rdfs:subClassOf rdf:resource="&java;JavaAPI"/>
		<rdfs:comment xml:lang="en">JavaLibrary implementing the org.apache.http.conn.scheme package for Android 2.3</rdfs:comment>
		<rdfs:comment xml:lang="OWLManchester">platform:comprisesInterfacePart some OrgApacheHttpConnScheme</rdfs:comment>
	</owl:Class>
	<owl:Class rdf:about="&android-2_3;OrgApacheHttpConnUtilAPI">
		<owl:equivalentClass rdf:resource="&android-2_2;OrgApacheHttpConnUtilAPI"/>
		<rdfs:subClassOf rdf:resource="&java;JavaAPI"/>
		<rdfs:comment xml:lang="en">JavaLibrary implementing the org.apache.http.conn.util package for Android 2.3</rdfs:comment>
		<rdfs:comment xml:lang="OWLManchester">platform:comprisesInterfacePart some OrgApacheHttpConnUtil</rdfs:comment>
	</owl:Class>
	<owl:Class rdf:about="&android-2_3;OrgApacheHttpConnParamsAPI">
		<owl:equivalentClass rdf:resource="&android-2_2;OrgApacheHttpConnParamsAPI"/>
		<rdfs:subClassOf rdf:resource="&java;JavaAPI"/>
		<rdfs:comment xml:lang="en">JavaLibrary implementing the org.apache.http.conn.params package for Android 2.3</rdfs:comment>
		<rdfs:comment xml:lang="OWLManchester">platform:comprisesInterfacePart some OrgApacheHttpConnParams</rdfs:comment>
	</owl:Class>
	<owl:Class rdf:about="&android-2_3;OrgApacheHttpProtocolAPI">
		<owl:equivalentClass rdf:resource="&android-2_2;OrgApacheHttpProtocolAPI"/>
		<rdfs:subClassOf rdf:resource="&java;JavaAPI"/>
		<rdfs:comment xml:lang="en">JavaLibrary implementing the org.apache.http.protocol package for Android 2.3</rdfs:comment>
		<rdfs:comment xml:lang="OWLManchester">platform:comprisesInterfacePart some OrgApacheHttpProtocol</rdfs:comment>
	</owl:Class>
	<owl:Class rdf:about="&android-2_3;OrgApacheHttpEntityAPI">
		<owl:equivalentClass rdf:resource="&android-2_2;OrgApacheHttpEntityAPI"/>
		<rdfs:subClassOf rdf:resource="&java;JavaAPI"/>
		<rdfs:comment xml:lang="en">JavaLibrary implementing the org.apache.http.entity package for Android 2.3</rdfs:comment>
		<rdfs:comment xml:lang="OWLManchester">platform:comprisesInterfacePart some OrgApacheHttpEntity</rdfs:comment>
	</owl:Class>
	<owl:Class rdf:about="&android-2_3;OrgApacheHttpImplAPI">
		<owl:equivalentClass rdf:resource="&android-2_2;OrgApacheHttpImplAPI"/>
		<rdfs:subClassOf rdf:resource="&java;JavaAPI"/>
		<rdfs:comment xml:lang="en">JavaLibrary implementing the org.apache.http.impl package for Android 2.3</rdfs:comment>
		<rdfs:comment xml:lang="OWLManchester">platform:comprisesInterfacePart some OrgApacheHttpImpl</rdfs:comment>
	</owl:Class>
	<owl:Class rdf:about="&android-2_3;OrgApacheHttpImplEntityAPI">
		<owl:equivalentClass rdf:resource="&android-2_2;OrgApacheHttpImplEntityAPI"/>
		<rdfs:subClassOf rdf:resource="&java;JavaAPI"/>
		<rdfs:comment xml:lang="en">JavaLibrary implementing the org.apache.http.impl.entity package for Android 2.3</rdfs:comment>
		<rdfs:comment xml:lang="OWLManchester">platform:comprisesInterfacePart some OrgApacheHttpImplEntity</rdfs:comment>
	</owl:Class>
	<owl:Class rdf:about="&android-2_3;OrgApacheHttpImplConnAPI">
		<owl:equivalentClass rdf:resource="&android-2_2;OrgApacheHttpImplConnAPI"/>
		<rdfs:subClassOf rdf:resource="&java;JavaAPI"/>
		<rdfs:comment xml:lang="en">JavaLibrary implementing the org.apache.http.impl.conn package for Android 2.3</rdfs:comment>
		<rdfs:comment xml:lang="OWLManchester">platform:comprisesInterfacePart some OrgApacheHttpImplConn</rdfs:comment>
	</owl:Class>
	<owl:Class rdf:about="&android-2_3;OrgApacheHttpImplConnTsccmAPI">
		<owl:equivalentClass rdf:resource="&android-2_2;OrgApacheHttpImplConnTsccmAPI"/>
		<rdfs:subClassOf rdf:resource="&java;JavaAPI"/>
		<rdfs:comment xml:lang="en">JavaLibrary implementing the org.apache.http.impl.conn.tsccm package for Android 2.3</rdfs:comment>
		<rdfs:comment xml:lang="OWLManchester">platform:comprisesInterfacePart some OrgApacheHttpImplConnTsccm</rdfs:comment>
	</owl:Class>
	<owl:Class rdf:about="&android-2_3;OrgApacheHttpImplIoAPI">
		<owl:equivalentClass rdf:resource="&android-2_2;OrgApacheHttpImplIoAPI"/>
		<rdfs:subClassOf rdf:resource="&java;JavaAPI"/>
		<rdfs:comment xml:lang="en">JavaLibrary implementing the org.apache.http.impl.io package for Android 2.3</rdfs:comment>
		<rdfs:comment xml:lang="OWLManchester">platform:comprisesInterfacePart some OrgApacheHttpImplIo</rdfs:comment>
	</owl:Class>
	<owl:Class rdf:about="&android-2_3;OrgApacheHttpImplCookieAPI">
		<owl:equivalentClass rdf:resource="&android-2_2;OrgApacheHttpImplCookieAPI"/>
		<rdfs:subClassOf rdf:resource="&java;JavaAPI"/>
		<rdfs:comment xml:lang="en">JavaLibrary implementing the org.apache.http.impl.cookie package for Android 2.3</rdfs:comment>
		<rdfs:comment xml:lang="OWLManchester">platform:comprisesInterfacePart some OrgApacheHttpImplCookie</rdfs:comment>
	</owl:Class>
	<owl:Class rdf:about="&android-2_3;OrgApacheHttpImplAuthAPI">
		<owl:equivalentClass rdf:resource="&android-2_2;OrgApacheHttpImplAuthAPI"/>
		<rdfs:subClassOf rdf:resource="&java;JavaAPI"/>
		<rdfs:comment xml:lang="en">JavaLibrary implementing the org.apache.http.impl.auth package for Android 2.3</rdfs:comment>
		<rdfs:comment xml:lang="OWLManchester">platform:comprisesInterfacePart some OrgApacheHttpImplAuth</rdfs:comment>
	</owl:Class>
	<owl:Class rdf:about="&android-2_3;OrgApacheHttpImplClientAPI">
		<owl:equivalentClass rdf:resource="&android-2_2;OrgApacheHttpImplClientAPI"/>
		<rdfs:subClassOf rdf:resource="&java;JavaAPI"/>
		<rdfs:comment xml:lang="en">JavaLibrary implementing the org.apache.http.impl.client package for Android 2.3</rdfs:comment>
		<rdfs:comment xml:lang="OWLManchester">platform:comprisesInterfacePart some OrgApacheHttpImplClient</rdfs:comment>
	</owl:Class>
	<owl:Class rdf:about="&android-2_3;OrgApacheHttpIoAPI">
		<owl:equivalentClass rdf:resource="&android-2_2;OrgApacheHttpIoAPI"/>
		<rdfs:subClassOf rdf:resource="&java;JavaAPI"/>
		<rdfs:comment xml:lang="en">JavaLibrary implementing the org.apache.http.io package for Android 2.3</rdfs:comment>
		<rdfs:comment xml:lang="OWLManchester">platform:comprisesInterfacePart some OrgApacheHttpIo</rdfs:comment>
	</owl:Class>
	<owl:Class rdf:about="&android-2_3;OrgApacheHttpUtilAPI">
		<owl:equivalentClass rdf:resource="&android-2_2;OrgApacheHttpUtilAPI"/>
		<rdfs:subClassOf rdf:resource="&java;JavaAPI"/>
		<rdfs:comment xml:lang="en">JavaLibrary implementing the org.apache.http.util package for Android 2.3</rdfs:comment>
		<rdfs:comment xml:lang="OWLManchester">platform:comprisesInterfacePart some OrgApacheHttpUtil</rdfs:comment>
	</owl:Class>
	<owl:Class rdf:about="&android-2_3;OrgApacheHttpMessageAPI">
		<owl:equivalentClass rdf:resource="&android-2_2;OrgApacheHttpMessageAPI"/>
		<rdfs:subClassOf rdf:resource="&java;JavaAPI"/>
		<rdfs:comment xml:lang="en">JavaLibrary implementing the org.apache.http.message package for Android 2.3</rdfs:comment>
		<rdfs:comment xml:lang="OWLManchester">platform:comprisesInterfacePart some OrgApacheHttpMessage</rdfs:comment>
	</owl:Class>
	<owl:Class rdf:about="&android-2_3;OrgApacheHttpCookieAPI">
		<owl:equivalentClass rdf:resource="&android-2_2;OrgApacheHttpCookieAPI"/>
		<rdfs:subClassOf rdf:resource="&java;JavaAPI"/>
		<rdfs:comment xml:lang="en">JavaLibrary implementing the org.apache.http.cookie package for Android 2.3</rdfs:comment>
		<rdfs:comment xml:lang="OWLManchester">platform:comprisesInterfacePart some OrgApacheHttpCookie</rdfs:comment>
	</owl:Class>
	<owl:Class rdf:about="&android-2_3;OrgApacheHttpCookieParamsAPI">
		<owl:equivalentClass rdf:resource="&android-2_2;OrgApacheHttpCookieParamsAPI"/>
		<rdfs:subClassOf rdf:resource="&java;JavaAPI"/>
		<rdfs:comment xml:lang="en">JavaLibrary implementing the org.apache.http.cookie.params package for Android 2.3</rdfs:comment>
		<rdfs:comment xml:lang="OWLManchester">platform:comprisesInterfacePart some OrgApacheHttpCookieParams</rdfs:comment>
	</owl:Class>
	<owl:Class rdf:about="&android-2_3;OrgApacheHttpAuthAPI">
		<owl:equivalentClass rdf:resource="&android-2_2;OrgApacheHttpAuthAPI"/>
		<rdfs:subClassOf rdf:resource="&java;JavaAPI"/>
		<rdfs:comment xml:lang="en">JavaLibrary implementing the org.apache.http.auth package for Android 2.3</rdfs:comment>
		<rdfs:comment xml:lang="OWLManchester">platform:comprisesInterfacePart some OrgApacheHttpAuth</rdfs:comment>
	</owl:Class>
	<owl:Class rdf:about="&android-2_3;OrgApacheHttpAuthParamsAPI">
		<owl:equivalentClass rdf:resource="&android-2_2;OrgApacheHttpAuthParamsAPI"/>
		<rdfs:subClassOf rdf:resource="&java;JavaAPI"/>
		<rdfs:comment xml:lang="en">JavaLibrary implementing the org.apache.http.auth.params package for Android 2.3</rdfs:comment>
		<rdfs:comment xml:lang="OWLManchester">platform:comprisesInterfacePart some OrgApacheHttpAuthParams</rdfs:comment>
	</owl:Class>
	<owl:Class rdf:about="&android-2_3;OrgApacheCommonsLoggingAPI">
		<owl:equivalentClass rdf:resource="&android-2_2;OrgApacheCommonsLoggingAPI"/>
		<rdfs:subClassOf rdf:resource="&java;JavaAPI"/>
		<rdfs:comment xml:lang="en">JavaLibrary implementing the org.apache.commons.logging package for Android 2.3</rdfs:comment>
		<rdfs:comment xml:lang="OWLManchester">platform:comprisesInterfacePart some OrgApacheCommonsLogging</rdfs:comment>
	</owl:Class>
	<owl:Class rdf:about="&android-2_3;OrgJsonAPI">
		<owl:equivalentClass rdf:resource="&android-2_2;OrgJsonAPI"/>
		<rdfs:subClassOf rdf:resource="&java;JavaAPI"/>
		<rdfs:comment xml:lang="en">JavaLibrary implementing the org.json package for Android 2.3</rdfs:comment>
		<rdfs:comment xml:lang="OWLManchester">platform:comprisesInterfacePart some OrgJson</rdfs:comment>
	</owl:Class>
	<owl:Class rdf:about="&android-2_3;DalvikBytecodeAPI">
		<rdfs:subClassOf rdf:resource="&android-2_2;DalvikBytecodeAPI"/>
		<rdfs:comment xml:lang="en">JavaLibrary implementing the dalvik.bytecode package for Android 2.3</rdfs:comment>
		<rdfs:comment xml:lang="OWLManchester">platform:comprisesInterfacePart some DalvikBytecode</rdfs:comment>
	</owl:Class>
	<owl:Class rdf:about="&android-2_3;DalvikAnnotationAPI">
		<owl:equivalentClass rdf:resource="&android-2_2;DalvikAnnotationAPI"/>
		<rdfs:subClassOf rdf:resource="&java;JavaAPI"/>
		<rdfs:comment xml:lang="en">JavaLibrary implementing the dalvik.annotation package for Android 2.3</rdfs:comment>
		<rdfs:comment xml:lang="OWLManchester">platform:comprisesInterfacePart some DalvikAnnotation</rdfs:comment>
	</owl:Class>
	<owl:Class rdf:about="&android-2_3;DalvikSystemAPI">
		<rdfs:subClassOf rdf:resource="&java;JavaAPI"/>
		<rdfs:comment xml:lang="en">JavaLibrary implementing the dalvik.system package for Android 2.3</rdfs:comment>
		<rdfs:comment xml:lang="OWLManchester">platform:comprisesInterfacePart some DalvikSystem</rdfs:comment>
	</owl:Class>
	<owl:Class rdf:about="&android-2_3;JunitRunnerAPI">
		<owl:equivalentClass rdf:resource="&android-2_2;JunitRunnerAPI"/>
		<rdfs:subClassOf rdf:resource="&java;JavaAPI"/>
		<rdfs:comment xml:lang="en">JavaLibrary implementing the junit.runner package for Android 2.3</rdfs:comment>
		<rdfs:comment xml:lang="OWLManchester">platform:comprisesInterfacePart some JunitRunner</rdfs:comment>
	</owl:Class>
	<owl:Class rdf:about="&android-2_3;JunitFrameworkAPI">
		<owl:equivalentClass rdf:resource="&android-2_2;JunitFrameworkAPI"/>
		<rdfs:subClassOf rdf:resource="&java;JavaAPI"/>
		<rdfs:comment xml:lang="en">JavaLibrary implementing the junit.framework package for Android 2.3</rdfs:comment>
		<rdfs:comment xml:lang="OWLManchester">platform:comprisesInterfacePart some JunitFramework</rdfs:comment>
	</owl:Class>
	<owl:Class rdf:about="&android-2_3;AndroidAPI">
		<rdfs:subClassOf rdf:resource="&java;JavaAPI"/>
		<rdfs:comment xml:lang="en">JavaLibrary implementing the android package for Android 2.3</rdfs:comment>
		<rdfs:comment xml:lang="OWLManchester">platform:comprisesInterfacePart some Android</rdfs:comment>
	</owl:Class>
	<owl:Class rdf:about="&android-2_3;AndroidContentAPI">
		<rdfs:subClassOf rdf:resource="&android-2_2;AndroidContentAPI"/>
		<rdfs:comment xml:lang="en">JavaLibrary implementing the android.content package for Android 2.3</rdfs:comment>
		<rdfs:comment xml:lang="OWLManchester">platform:comprisesInterfacePart some AndroidContent</rdfs:comment>
	</owl:Class>
	<owl:Class rdf:about="&android-2_3;AndroidContentPmAPI">
		<rdfs:subClassOf rdf:resource="&android-2_2;AndroidContentPmAPI"/>
		<rdfs:comment xml:lang="en">JavaLibrary implementing the android.content.pm package for Android 2.3</rdfs:comment>
		<rdfs:comment xml:lang="OWLManchester">platform:comprisesInterfacePart some AndroidContentPm</rdfs:comment>
	</owl:Class>
	<owl:Class rdf:about="&android-2_3;AndroidContentResAPI">
		<rdfs:subClassOf rdf:resource="&android-2_2;AndroidContentResAPI"/>
		<rdfs:comment xml:lang="en">JavaLibrary implementing the android.content.res package for Android 2.3</rdfs:comment>
		<rdfs:comment xml:lang="OWLManchester">platform:comprisesInterfacePart some AndroidContentRes</rdfs:comment>
	</owl:Class>
	<owl:Class rdf:about="&android-2_3;AndroidOsAPI">
		<rdfs:subClassOf rdf:resource="&android-2_2;AndroidOsAPI"/>
		<rdfs:comment xml:lang="en">JavaLibrary implementing the android.os package for Android 2.3</rdfs:comment>
		<rdfs:comment xml:lang="OWLManchester">platform:comprisesInterfacePart some AndroidOs</rdfs:comment>
	</owl:Class>
	<owl:Class rdf:about="&android-2_3;AndroidOsStorageAPI">
		<rdfs:subClassOf rdf:resource="&java;JavaAPI"/>
		<rdfs:comment xml:lang="en">JavaLibrary implementing the android.os.storage package for Android 2.3</rdfs:comment>
		<rdfs:comment xml:lang="OWLManchester">platform:comprisesInterfacePart some AndroidOsStorage</rdfs:comment>
	</owl:Class>
	<owl:Class rdf:about="&android-2_3;AndroidAccountsAPI">
		<rdfs:subClassOf rdf:resource="&android-2_2;AndroidAccountsAPI"/>
		<rdfs:comment xml:lang="en">JavaLibrary implementing the android.accounts package for Android 2.3</rdfs:comment>
		<rdfs:comment xml:lang="OWLManchester">platform:comprisesInterfacePart some AndroidAccounts</rdfs:comment>
	</owl:Class>
	<owl:Class rdf:about="&android-2_3;AndroidNetAPI">
		<rdfs:subClassOf rdf:resource="&android-2_2;AndroidNetAPI"/>
		<rdfs:comment xml:lang="en">JavaLibrary implementing the android.net package for Android 2.3</rdfs:comment>
		<rdfs:comment xml:lang="OWLManchester">platform:comprisesInterfacePart some AndroidNet</rdfs:comment>
	</owl:Class>
	<owl:Class rdf:about="&android-2_3;AndroidNetHttpAPI">
		<owl:equivalentClass rdf:resource="&android-2_2;AndroidNetHttpAPI"/>
		<rdfs:subClassOf rdf:resource="&java;JavaAPI"/>
		<rdfs:comment xml:lang="en">JavaLibrary implementing the android.net.http package for Android 2.3</rdfs:comment>
		<rdfs:comment xml:lang="OWLManchester">platform:comprisesInterfacePart some AndroidNetHttp</rdfs:comment>
	</owl:Class>
	<owl:Class rdf:about="&android-2_3;AndroidNetSipAPI">
		<rdfs:subClassOf rdf:resource="&java;JavaAPI"/>
		<rdfs:comment xml:lang="en">JavaLibrary implementing the android.net.sip package for Android 2.3</rdfs:comment>
		<rdfs:comment xml:lang="OWLManchester">platform:comprisesInterfacePart some AndroidNetSip</rdfs:comment>
	</owl:Class>
	<owl:Class rdf:about="&android-2_3;AndroidNetWifiAPI">
		<rdfs:subClassOf rdf:resource="&android-2_2;AndroidNetWifiAPI"/>
		<rdfs:comment xml:lang="en">JavaLibrary implementing the android.net.wifi package for Android 2.3</rdfs:comment>
		<rdfs:comment xml:lang="OWLManchester">platform:comprisesInterfacePart some AndroidNetWifi</rdfs:comment>
	</owl:Class>
	<owl:Class rdf:about="&android-2_3;AndroidDatabaseAPI">
		<rdfs:subClassOf rdf:resource="&android-2_2;AndroidDatabaseAPI"/>
		<rdfs:comment xml:lang="en">JavaLibrary implementing the android.database package for Android 2.3</rdfs:comment>
		<rdfs:comment xml:lang="OWLManchester">platform:comprisesInterfacePart some AndroidDatabase</rdfs:comment>
	</owl:Class>
	<owl:Class rdf:about="&android-2_3;AndroidDatabaseSqliteAPI">
		<owl:equivalentClass rdf:resource="&android-2_2;AndroidDatabaseSqliteAPI"/>
		<rdfs:subClassOf rdf:resource="&java;JavaAPI"/>
		<rdfs:comment xml:lang="en">JavaLibrary implementing the android.database.sqlite package for Android 2.3</rdfs:comment>
		<rdfs:comment xml:lang="OWLManchester">platform:comprisesInterfacePart some AndroidDatabaseSqlite</rdfs:comment>
	</owl:Class>
	<owl:Class rdf:about="&android-2_3;AndroidUtilAPI">
		<rdfs:subClassOf rdf:resource="&android-2_2;AndroidUtilAPI"/>
		<rdfs:comment xml:lang="en">JavaLibrary implementing the android.util package for Android 2.3</rdfs:comment>
		<rdfs:comment xml:lang="OWLManchester">platform:comprisesInterfacePart some AndroidUtil</rdfs:comment>
	</owl:Class>
	<owl:Class rdf:about="&android-2_3;AndroidGraphicsAPI">
		<rdfs:subClassOf rdf:resource="&android-2_2;AndroidGraphicsAPI"/>
		<rdfs:comment xml:lang="en">JavaLibrary implementing the android.graphics package for Android 2.3</rdfs:comment>
		<rdfs:comment xml:lang="OWLManchester">platform:comprisesInterfacePart some AndroidGraphics</rdfs:comment>
	</owl:Class>
	<owl:Class rdf:about="&android-2_3;AndroidGraphicsDrawableAPI">
		<rdfs:subClassOf rdf:resource="&android-2_2;AndroidGraphicsDrawableAPI"/>
		<rdfs:comment xml:lang="en">JavaLibrary implementing the android.graphics.drawable package for Android 2.3</rdfs:comment>
		<rdfs:comment xml:lang="OWLManchester">platform:comprisesInterfacePart some AndroidGraphicsDrawable</rdfs:comment>
	</owl:Class>
	<owl:Class rdf:about="&android-2_3;AndroidGraphicsDrawableShapesAPI">
		<owl:equivalentClass rdf:resource="&android-2_2;AndroidGraphicsDrawableShapesAPI"/>
		<rdfs:subClassOf rdf:resource="&java;JavaAPI"/>
		<rdfs:comment xml:lang="en">JavaLibrary implementing the android.graphics.drawable.shapes package for Android 2.3</rdfs:comment>
		<rdfs:comment xml:lang="OWLManchester">platform:comprisesInterfacePart some AndroidGraphicsDrawableShapes</rdfs:comment>
	</owl:Class>
	<owl:Class rdf:about="&android-2_3;AndroidViewAPI">
		<rdfs:subClassOf rdf:resource="&java;JavaAPI"/>
		<rdfs:comment xml:lang="en">JavaLibrary implementing the android.view package for Android 2.3</rdfs:comment>
		<rdfs:comment xml:lang="OWLManchester">platform:comprisesInterfacePart some AndroidView</rdfs:comment>
	</owl:Class>
	<owl:Class rdf:about="&android-2_3;AndroidViewAccessibilityAPI">
		<owl:equivalentClass rdf:resource="&android-2_2;AndroidViewAccessibilityAPI"/>
		<rdfs:subClassOf rdf:resource="&java;JavaAPI"/>
		<rdfs:comment xml:lang="en">JavaLibrary implementing the android.view.accessibility package for Android 2.3</rdfs:comment>
		<rdfs:comment xml:lang="OWLManchester">platform:comprisesInterfacePart some AndroidViewAccessibility</rdfs:comment>
	</owl:Class>
	<owl:Class rdf:about="&android-2_3;AndroidViewInputmethodAPI">
		<rdfs:subClassOf rdf:resource="&android-2_2;AndroidViewInputmethodAPI"/>
		<rdfs:comment xml:lang="en">JavaLibrary implementing the android.view.inputmethod package for Android 2.3</rdfs:comment>
		<rdfs:comment xml:lang="OWLManchester">platform:comprisesInterfacePart some AndroidViewInputmethod</rdfs:comment>
	</owl:Class>
	<owl:Class rdf:about="&android-2_3;AndroidViewAnimationAPI">
		<owl:equivalentClass rdf:resource="&android-2_2;AndroidViewAnimationAPI"/>
		<rdfs:subClassOf rdf:resource="&java;JavaAPI"/>
		<rdfs:comment xml:lang="en">JavaLibrary implementing the android.view.animation package for Android 2.3</rdfs:comment>
		<rdfs:comment xml:lang="OWLManchester">platform:comprisesInterfacePart some AndroidViewAnimation</rdfs:comment>
	</owl:Class>
	<owl:Class rdf:about="&android-2_3;AndroidAccessibilityserviceAPI">
		<rdfs:subClassOf rdf:resource="&android-2_2;AndroidAccessibilityserviceAPI"/>
		<rdfs:comment xml:lang="en">JavaLibrary implementing the android.accessibilityservice package for Android 2.3</rdfs:comment>
		<rdfs:comment xml:lang="OWLManchester">platform:comprisesInterfacePart some AndroidAccessibilityservice</rdfs:comment>
	</owl:Class>
	<owl:Class rdf:about="&android-2_3;AndroidAppAPI">
		<rdfs:subClassOf rdf:resource="&android-2_2;AndroidAppAPI"/>
		<rdfs:comment xml:lang="en">JavaLibrary implementing the android.app package for Android 2.3</rdfs:comment>
		<rdfs:comment xml:lang="OWLManchester">platform:comprisesInterfacePart some AndroidApp</rdfs:comment>
	</owl:Class>
	<owl:Class rdf:about="&android-2_3;AndroidAppBackupAPI">
		<rdfs:subClassOf rdf:resource="&android-2_2;AndroidAppBackupAPI"/>
		<rdfs:comment xml:lang="en">JavaLibrary implementing the android.app.backup package for Android 2.3</rdfs:comment>
		<rdfs:comment xml:lang="OWLManchester">platform:comprisesInterfacePart some AndroidAppBackup</rdfs:comment>
	</owl:Class>
	<owl:Class rdf:about="&android-2_3;AndroidAppAdminAPI">
		<rdfs:subClassOf rdf:resource="&android-2_2;AndroidAppAdminAPI"/>
		<rdfs:comment xml:lang="en">JavaLibrary implementing the android.app.admin package for Android 2.3</rdfs:comment>
		<rdfs:comment xml:lang="OWLManchester">platform:comprisesInterfacePart some AndroidAppAdmin</rdfs:comment>
	</owl:Class>
	<owl:Class rdf:about="&android-2_3;AndroidTelephonyAPI">
		<rdfs:subClassOf rdf:resource="&android-2_2;AndroidTelephonyAPI"/>
		<rdfs:comment xml:lang="en">JavaLibrary implementing the android.telephony package for Android 2.3</rdfs:comment>
		<rdfs:comment xml:lang="OWLManchester">platform:comprisesInterfacePart some AndroidTelephony</rdfs:comment>
	</owl:Class>
	<owl:Class rdf:about="&android-2_3;AndroidTelephonyCdmaAPI">
		<owl:equivalentClass rdf:resource="&android-2_2;AndroidTelephonyCdmaAPI"/>
		<rdfs:subClassOf rdf:resource="&java;JavaAPI"/>
		<rdfs:comment xml:lang="en">JavaLibrary implementing the android.telephony.cdma package for Android 2.3</rdfs:comment>
		<rdfs:comment xml:lang="OWLManchester">platform:comprisesInterfacePart some AndroidTelephonyCdma</rdfs:comment>
	</owl:Class>
	<owl:Class rdf:about="&android-2_3;AndroidTelephonyGsmAPI">
		<rdfs:subClassOf rdf:resource="&android-2_2;AndroidTelephonyGsmAPI"/>
		<rdfs:comment xml:lang="en">JavaLibrary implementing the android.telephony.gsm package for Android 2.3</rdfs:comment>
		<rdfs:comment xml:lang="OWLManchester">platform:comprisesInterfacePart some AndroidTelephonyGsm</rdfs:comment>
	</owl:Class>
	<owl:Class rdf:about="&android-2_3;AndroidTextAPI">
		<rdfs:subClassOf rdf:resource="&android-2_2;AndroidTextAPI"/>
		<rdfs:comment xml:lang="en">JavaLibrary implementing the android.text package for Android 2.3</rdfs:comment>
		<rdfs:comment xml:lang="OWLManchester">platform:comprisesInterfacePart some AndroidText</rdfs:comment>
	</owl:Class>
	<owl:Class rdf:about="&android-2_3;AndroidTextUtilAPI">
		<owl:equivalentClass rdf:resource="&android-2_2;AndroidTextUtilAPI"/>
		<rdfs:subClassOf rdf:resource="&java;JavaAPI"/>
		<rdfs:comment xml:lang="en">JavaLibrary implementing the android.text.util package for Android 2.3</rdfs:comment>
		<rdfs:comment xml:lang="OWLManchester">platform:comprisesInterfacePart some AndroidTextUtil</rdfs:comment>
	</owl:Class>
	<owl:Class rdf:about="&android-2_3;AndroidTextFormatAPI">
		<rdfs:subClassOf rdf:resource="&android-2_2;AndroidTextFormatAPI"/>
		<rdfs:comment xml:lang="en">JavaLibrary implementing the android.text.format package for Android 2.3</rdfs:comment>
		<rdfs:comment xml:lang="OWLManchester">platform:comprisesInterfacePart some AndroidTextFormat</rdfs:comment>
	</owl:Class>
	<owl:Class rdf:about="&android-2_3;AndroidTextMethodAPI">
		<rdfs:subClassOf rdf:resource="&android-2_2;AndroidTextMethodAPI"/>
		<rdfs:comment xml:lang="en">JavaLibrary implementing the android.text.method package for Android 2.3</rdfs:comment>
		<rdfs:comment xml:lang="OWLManchester">platform:comprisesInterfacePart some AndroidTextMethod</rdfs:comment>
	</owl:Class>
	<owl:Class rdf:about="&android-2_3;AndroidTextStyleAPI">
		<owl:equivalentClass rdf:resource="&android-2_2;AndroidTextStyleAPI"/>
		<rdfs:subClassOf rdf:resource="&java;JavaAPI"/>
		<rdfs:comment xml:lang="en">JavaLibrary implementing the android.text.style package for Android 2.3</rdfs:comment>
		<rdfs:comment xml:lang="OWLManchester">platform:comprisesInterfacePart some AndroidTextStyle</rdfs:comment>
	</owl:Class>
	<owl:Class rdf:about="&android-2_3;AndroidGestureAPI">
		<rdfs:subClassOf rdf:resource="&android-2_2;AndroidGestureAPI"/>
		<rdfs:comment xml:lang="en">JavaLibrary implementing the android.gesture package for Android 2.3</rdfs:comment>
		<rdfs:comment xml:lang="OWLManchester">platform:comprisesInterfacePart some AndroidGesture</rdfs:comment>
	</owl:Class>
	<owl:Class rdf:about="&android-2_3;AndroidWidgetAPI">
		<rdfs:subClassOf rdf:resource="&android-2_2;AndroidWidgetAPI"/>
		<rdfs:comment xml:lang="en">JavaLibrary implementing the android.widget package for Android 2.3</rdfs:comment>
		<rdfs:comment xml:lang="OWLManchester">platform:comprisesInterfacePart some AndroidWidget</rdfs:comment>
	</owl:Class>
	<owl:Class rdf:about="&android-2_3;AndroidLocationAPI">
		<rdfs:subClassOf rdf:resource="&android-2_2;AndroidLocationAPI"/>
		<rdfs:comment xml:lang="en">JavaLibrary implementing the android.location package for Android 2.3</rdfs:comment>
		<rdfs:comment xml:lang="OWLManchester">platform:comprisesInterfacePart some AndroidLocation</rdfs:comment>
	</owl:Class>
	<owl:Class rdf:about="&android-2_3;AndroidHardwareAPI">
		<rdfs:subClassOf rdf:resource="&android-2_2;AndroidHardwareAPI"/>
		<rdfs:comment xml:lang="en">JavaLibrary implementing the android.hardware package for Android 2.3</rdfs:comment>
		<rdfs:comment xml:lang="OWLManchester">platform:comprisesInterfacePart some AndroidHardware</rdfs:comment>
	</owl:Class>
	<owl:Class rdf:about="&android-2_3;AndroidWebkitAPI">
		<rdfs:subClassOf rdf:resource="&android-2_2;AndroidWebkitAPI"/>
		<rdfs:comment xml:lang="en">JavaLibrary implementing the android.webkit package for Android 2.3</rdfs:comment>
		<rdfs:comment xml:lang="OWLManchester">platform:comprisesInterfacePart some AndroidWebkit</rdfs:comment>
	</owl:Class>
	<owl:Class rdf:about="&android-2_3;AndroidTestAPI">
		<rdfs:subClassOf rdf:resource="&android-2_2;AndroidTestAPI"/>
		<rdfs:comment xml:lang="en">JavaLibrary implementing the android.test package for Android 2.3</rdfs:comment>
		<rdfs:comment xml:lang="OWLManchester">platform:comprisesInterfacePart some AndroidTest</rdfs:comment>
	</owl:Class>
	<owl:Class rdf:about="&android-2_3;AndroidTestMockAPI">
		<rdfs:subClassOf rdf:resource="&android-2_2;AndroidTestMockAPI"/>
		<rdfs:comment xml:lang="en">JavaLibrary implementing the android.test.mock package for Android 2.3</rdfs:comment>
		<rdfs:comment xml:lang="OWLManchester">platform:comprisesInterfacePart some AndroidTestMock</rdfs:comment>
	</owl:Class>
	<owl:Class rdf:about="&android-2_3;AndroidTestSuitebuilderAPI">
		<owl:equivalentClass rdf:resource="&android-2_2;AndroidTestSuitebuilderAPI"/>
		<rdfs:subClassOf rdf:resource="&java;JavaAPI"/>
		<rdfs:comment xml:lang="en">JavaLibrary implementing the android.test.suitebuilder package for Android 2.3</rdfs:comment>
		<rdfs:comment xml:lang="OWLManchester">platform:comprisesInterfacePart some AndroidTestSuitebuilder</rdfs:comment>
	</owl:Class>
	<owl:Class rdf:about="&android-2_3;AndroidTestSuitebuilderAnnotationAPI">
		<owl:equivalentClass rdf:resource="&android-2_2;AndroidTestSuitebuilderAnnotationAPI"/>
		<rdfs:subClassOf rdf:resource="&java;JavaAPI"/>
		<rdfs:comment xml:lang="en">JavaLibrary implementing the android.test.suitebuilder.annotation package for Android 2.3</rdfs:comment>
		<rdfs:comment xml:lang="OWLManchester">platform:comprisesInterfacePart some AndroidTestSuitebuilderAnnotation</rdfs:comment>
	</owl:Class>
	<owl:Class rdf:about="&android-2_3;AndroidPreferenceAPI">
		<rdfs:subClassOf rdf:resource="&android-2_2;AndroidPreferenceAPI"/>
		<rdfs:comment xml:lang="en">JavaLibrary implementing the android.preference package for Android 2.3</rdfs:comment>
		<rdfs:comment xml:lang="OWLManchester">platform:comprisesInterfacePart some AndroidPreference</rdfs:comment>
	</owl:Class>
	<owl:Class rdf:about="&android-2_3;AndroidMediaAPI">
		<rdfs:subClassOf rdf:resource="&android-2_2;AndroidMediaAPI"/>
		<rdfs:comment xml:lang="en">JavaLibrary implementing the android.media package for Android 2.3</rdfs:comment>
		<rdfs:comment xml:lang="OWLManchester">platform:comprisesInterfacePart some AndroidMedia</rdfs:comment>
	</owl:Class>
	<owl:Class rdf:about="&android-2_3;AndroidMediaAudiofxAPI">
		<rdfs:subClassOf rdf:resource="&java;JavaAPI"/>
		<rdfs:comment xml:lang="en">JavaLibrary implementing the android.media.audiofx package for Android 2.3</rdfs:comment>
		<rdfs:comment xml:lang="OWLManchester">platform:comprisesInterfacePart some AndroidMediaAudiofx</rdfs:comment>
	</owl:Class>
	<owl:Class rdf:about="&android-2_3;AndroidInputmethodserviceAPI">
		<rdfs:subClassOf rdf:resource="&android-2_2;AndroidInputmethodserviceAPI"/>
		<rdfs:comment xml:lang="en">JavaLibrary implementing the android.inputmethodservice package for Android 2.3</rdfs:comment>
		<rdfs:comment xml:lang="OWLManchester">platform:comprisesInterfacePart some AndroidInputmethodservice</rdfs:comment>
	</owl:Class>
	<owl:Class rdf:about="&android-2_3;AndroidServiceWallpaperAPI">
		<rdfs:subClassOf rdf:resource="&android-2_2;AndroidServiceWallpaperAPI"/>
		<rdfs:comment xml:lang="en">JavaLibrary implementing the android.service.wallpaper package for Android 2.3</rdfs:comment>
		<rdfs:comment xml:lang="OWLManchester">platform:comprisesInterfacePart some AndroidServiceWallpaper</rdfs:comment>
	</owl:Class>
	<owl:Class rdf:about="&android-2_3;AndroidBluetoothAPI">
		<owl:equivalentClass rdf:resource="&android-2_2;AndroidBluetoothAPI"/>
		<rdfs:subClassOf rdf:resource="&java;JavaAPI"/>
		<rdfs:comment xml:lang="en">JavaLibrary implementing the android.bluetooth package for Android 2.3</rdfs:comment>
		<rdfs:comment xml:lang="OWLManchester">platform:comprisesInterfacePart some AndroidBluetooth</rdfs:comment>
	</owl:Class>
	<owl:Class rdf:about="&android-2_3;AndroidNfcAPI">
		<rdfs:subClassOf rdf:resource="&java;JavaAPI"/>
		<rdfs:comment xml:lang="en">JavaLibrary implementing the android.nfc package for Android 2.3</rdfs:comment>
		<rdfs:comment xml:lang="OWLManchester">platform:comprisesInterfacePart some AndroidNfc</rdfs:comment>
	</owl:Class>
	<owl:Class rdf:about="&android-2_3;AndroidProviderAPI">
		<rdfs:subClassOf rdf:resource="&android-2_2;AndroidProviderAPI"/>
		<rdfs:comment xml:lang="en">JavaLibrary implementing the android.provider package for Android 2.3</rdfs:comment>
		<rdfs:comment xml:lang="OWLManchester">platform:comprisesInterfacePart some AndroidProvider</rdfs:comment>
	</owl:Class>
	<owl:Class rdf:about="&android-2_3;AndroidSaxAPI">
		<owl:equivalentClass rdf:resource="&android-2_2;AndroidSaxAPI"/>
		<rdfs:subClassOf rdf:resource="&java;JavaAPI"/>
		<rdfs:comment xml:lang="en">JavaLibrary implementing the android.sax package for Android 2.3</rdfs:comment>
		<rdfs:comment xml:lang="OWLManchester">platform:comprisesInterfacePart some AndroidSax</rdfs:comment>
	</owl:Class>
	<owl:Class rdf:about="&android-2_3;AndroidAppwidgetAPI">
		<rdfs:subClassOf rdf:resource="&android-2_2;AndroidAppwidgetAPI"/>
		<rdfs:comment xml:lang="en">JavaLibrary implementing the android.appwidget package for Android 2.3</rdfs:comment>
		<rdfs:comment xml:lang="OWLManchester">platform:comprisesInterfacePart some AndroidAppwidget</rdfs:comment>
	</owl:Class>
	<owl:Class rdf:about="&android-2_3;AndroidOpenglAPI">
		<rdfs:subClassOf rdf:resource="&android-2_2;AndroidOpenglAPI"/>
		<rdfs:comment xml:lang="en">JavaLibrary implementing the android.opengl package for Android 2.3</rdfs:comment>
		<rdfs:comment xml:lang="OWLManchester">platform:comprisesInterfacePart some AndroidOpengl</rdfs:comment>
	</owl:Class>
	<owl:Class rdf:about="&android-2_3;AndroidSpeechAPI">
		<rdfs:subClassOf rdf:resource="&android-2_2;AndroidSpeechAPI"/>
		<rdfs:comment xml:lang="en">JavaLibrary implementing the android.speech package for Android 2.3</rdfs:comment>
		<rdfs:comment xml:lang="OWLManchester">platform:comprisesInterfacePart some AndroidSpeech</rdfs:comment>
	</owl:Class>
	<owl:Class rdf:about="&android-2_3;AndroidSpeechTtsAPI">
		<owl:equivalentClass rdf:resource="&android-2_2;AndroidSpeechTtsAPI"/>
		<rdfs:subClassOf rdf:resource="&java;JavaAPI"/>
		<rdfs:comment xml:lang="en">JavaLibrary implementing the android.speech.tts package for Android 2.3</rdfs:comment>
		<rdfs:comment xml:lang="OWLManchester">platform:comprisesInterfacePart some AndroidSpeechTts</rdfs:comment>
	</owl:Class>
	<android-2_3:JavaxXml rdf:about="&android-2_3;theJavaxXmlPart">
	</android-2_3:JavaxXml>
	<android-2_3:JavaxXmlDatatype rdf:about="&android-2_3;theJavaxXmlDatatypePart">
	</android-2_3:JavaxXmlDatatype>
	<android-2_3:JavaxXmlNamespace rdf:about="&android-2_3;theJavaxXmlNamespacePart">
	</android-2_3:JavaxXmlNamespace>
	<android-2_3:JavaxXmlXpath rdf:about="&android-2_3;theJavaxXmlXpathPart">
	</android-2_3:JavaxXmlXpath>
	<android-2_3:JavaxXmlTransform rdf:about="&android-2_3;theJavaxXmlTransformPart">
	</android-2_3:JavaxXmlTransform>
	<android-2_3:JavaxXmlTransformDom rdf:about="&android-2_3;theJavaxXmlTransformDomPart">
	</android-2_3:JavaxXmlTransformDom>
	<android-2_3:JavaxXmlTransformSax rdf:about="&android-2_3;theJavaxXmlTransformSaxPart">
	</android-2_3:JavaxXmlTransformSax>
	<android-2_3:JavaxXmlTransformStream rdf:about="&android-2_3;theJavaxXmlTransformStreamPart">
	</android-2_3:JavaxXmlTransformStream>
	<android-2_3:JavaxXmlParsers rdf:about="&android-2_3;theJavaxXmlParsersPart">
	</android-2_3:JavaxXmlParsers>
	<android-2_3:JavaxXmlValidation rdf:about="&android-2_3;theJavaxXmlValidationPart">
	</android-2_3:JavaxXmlValidation>
	<android-2_3:JavaxSecurityCert rdf:about="&android-2_3;theJavaxSecurityCertPart">
	</android-2_3:JavaxSecurityCert>
	<android-2_3:JavaxSecurityAuth rdf:about="&android-2_3;theJavaxSecurityAuthPart">
	</android-2_3:JavaxSecurityAuth>
	<android-2_3:JavaxSecurityAuthCallback rdf:about="&android-2_3;theJavaxSecurityAuthCallbackPart">
	</android-2_3:JavaxSecurityAuthCallback>
	<android-2_3:JavaxSecurityAuthLogin rdf:about="&android-2_3;theJavaxSecurityAuthLoginPart">
	</android-2_3:JavaxSecurityAuthLogin>
	<android-2_3:JavaxSecurityAuthX500 rdf:about="&android-2_3;theJavaxSecurityAuthX500Part">
	</android-2_3:JavaxSecurityAuthX500>
	<android-2_3:JavaxSql rdf:about="&android-2_3;theJavaxSqlPart">
	</android-2_3:JavaxSql>
	<android-2_3:JavaxCrypto rdf:about="&android-2_3;theJavaxCryptoPart">
	</android-2_3:JavaxCrypto>
	<android-2_3:JavaxCryptoInterfaces rdf:about="&android-2_3;theJavaxCryptoInterfacesPart">
	</android-2_3:JavaxCryptoInterfaces>
	<android-2_3:JavaxCryptoSpec rdf:about="&android-2_3;theJavaxCryptoSpecPart">
	</android-2_3:JavaxCryptoSpec>
	<android-2_3:JavaxMicroeditionKhronosEgl rdf:about="&android-2_3;theJavaxMicroeditionKhronosEglPart">
	</android-2_3:JavaxMicroeditionKhronosEgl>
	<android-2_3:JavaxMicroeditionKhronosOpengles rdf:about="&android-2_3;theJavaxMicroeditionKhronosOpenglesPart">
	</android-2_3:JavaxMicroeditionKhronosOpengles>
	<android-2_3:JavaxNet rdf:about="&android-2_3;theJavaxNetPart">
	</android-2_3:JavaxNet>
	<android-2_3:JavaxNetSsl rdf:about="&android-2_3;theJavaxNetSslPart">
	</android-2_3:JavaxNetSsl>
	<android-2_3:JavaLang rdf:about="&android-2_3;theJavaLangPart">
	</android-2_3:JavaLang>
	<android-2_3:JavaLangReflect rdf:about="&android-2_3;theJavaLangReflectPart">
	</android-2_3:JavaLangReflect>
	<android-2_3:JavaLangAnnotation rdf:about="&android-2_3;theJavaLangAnnotationPart">
	</android-2_3:JavaLangAnnotation>
	<android-2_3:JavaLangRef rdf:about="&android-2_3;theJavaLangRefPart">
	</android-2_3:JavaLangRef>
	<android-2_3:JavaUtil rdf:about="&android-2_3;theJavaUtilPart">
	</android-2_3:JavaUtil>
	<android-2_3:JavaUtilJar rdf:about="&android-2_3;theJavaUtilJarPart">
	</android-2_3:JavaUtilJar>
	<android-2_3:JavaUtilZip rdf:about="&android-2_3;theJavaUtilZipPart">
	</android-2_3:JavaUtilZip>
	<android-2_3:JavaUtilPrefs rdf:about="&android-2_3;theJavaUtilPrefsPart">
	</android-2_3:JavaUtilPrefs>
	<android-2_3:JavaUtilRegex rdf:about="&android-2_3;theJavaUtilRegexPart">
	</android-2_3:JavaUtilRegex>
	<android-2_3:JavaUtilConcurrent rdf:about="&android-2_3;theJavaUtilConcurrentPart">
	</android-2_3:JavaUtilConcurrent>
	<android-2_3:JavaUtilConcurrentAtomic rdf:about="&android-2_3;theJavaUtilConcurrentAtomicPart">
	</android-2_3:JavaUtilConcurrentAtomic>
	<android-2_3:JavaUtilConcurrentLocks rdf:about="&android-2_3;theJavaUtilConcurrentLocksPart">
	</android-2_3:JavaUtilConcurrentLocks>
	<android-2_3:JavaUtilLogging rdf:about="&android-2_3;theJavaUtilLoggingPart">
	</android-2_3:JavaUtilLogging>
	<android-2_3:JavaMath rdf:about="&android-2_3;theJavaMathPart">
	</android-2_3:JavaMath>
	<android-2_3:JavaIo rdf:about="&android-2_3;theJavaIoPart">
	</android-2_3:JavaIo>
	<android-2_3:JavaNet rdf:about="&android-2_3;theJavaNetPart">
	</android-2_3:JavaNet>
	<android-2_3:JavaSecurity rdf:about="&android-2_3;theJavaSecurityPart">
	</android-2_3:JavaSecurity>
	<android-2_3:JavaSecuritySpec rdf:about="&android-2_3;theJavaSecuritySpecPart">
	</android-2_3:JavaSecuritySpec>
	<android-2_3:JavaSecurityCert rdf:about="&android-2_3;theJavaSecurityCertPart">
	</android-2_3:JavaSecurityCert>
	<android-2_3:JavaSecurityInterfaces rdf:about="&android-2_3;theJavaSecurityInterfacesPart">
	</android-2_3:JavaSecurityInterfaces>
	<android-2_3:JavaSecurityAcl rdf:about="&android-2_3;theJavaSecurityAclPart">
	</android-2_3:JavaSecurityAcl>
	<android-2_3:JavaSql rdf:about="&android-2_3;theJavaSqlPart">
	</android-2_3:JavaSql>
	<android-2_3:JavaNio rdf:about="&android-2_3;theJavaNioPart">
	</android-2_3:JavaNio>
	<android-2_3:JavaNioChannels rdf:about="&android-2_3;theJavaNioChannelsPart">
	</android-2_3:JavaNioChannels>
	<android-2_3:JavaNioChannelsSpi rdf:about="&android-2_3;theJavaNioChannelsSpiPart">
	</android-2_3:JavaNioChannelsSpi>
	<android-2_3:JavaNioCharset rdf:about="&android-2_3;theJavaNioCharsetPart">
	</android-2_3:JavaNioCharset>
	<android-2_3:JavaNioCharsetSpi rdf:about="&android-2_3;theJavaNioCharsetSpiPart">
	</android-2_3:JavaNioCharsetSpi>
	<android-2_3:JavaBeans rdf:about="&android-2_3;theJavaBeansPart">
	</android-2_3:JavaBeans>
	<android-2_3:JavaText rdf:about="&android-2_3;theJavaTextPart">
	</android-2_3:JavaText>
	<android-2_3:JavaAwtFont rdf:about="&android-2_3;theJavaAwtFontPart">
	</android-2_3:JavaAwtFont>
	<android-2_3:OrgXmlSax rdf:about="&android-2_3;theOrgXmlSaxPart">
	</android-2_3:OrgXmlSax>
	<android-2_3:OrgXmlSaxExt rdf:about="&android-2_3;theOrgXmlSaxExtPart">
	</android-2_3:OrgXmlSaxExt>
	<android-2_3:OrgXmlSaxHelpers rdf:about="&android-2_3;theOrgXmlSaxHelpersPart">
	</android-2_3:OrgXmlSaxHelpers>
	<android-2_3:OrgW3cDom rdf:about="&android-2_3;theOrgW3cDomPart">
	</android-2_3:OrgW3cDom>
	<android-2_3:OrgW3cDomLs rdf:about="&android-2_3;theOrgW3cDomLsPart">
	</android-2_3:OrgW3cDomLs>
	<android-2_3:OrgXmlpullV1 rdf:about="&android-2_3;theOrgXmlpullV1Part">
	</android-2_3:OrgXmlpullV1>
	<android-2_3:OrgXmlpullV1Sax2 rdf:about="&android-2_3;theOrgXmlpullV1Sax2Part">
	</android-2_3:OrgXmlpullV1Sax2>
	<android-2_3:OrgApacheHttp rdf:about="&android-2_3;theOrgApacheHttpPart">
	</android-2_3:OrgApacheHttp>
	<android-2_3:OrgApacheHttpClient rdf:about="&android-2_3;theOrgApacheHttpClientPart">
	</android-2_3:OrgApacheHttpClient>
	<android-2_3:OrgApacheHttpClientMethods rdf:about="&android-2_3;theOrgApacheHttpClientMethodsPart">
	</android-2_3:OrgApacheHttpClientMethods>
	<android-2_3:OrgApacheHttpClientEntity rdf:about="&android-2_3;theOrgApacheHttpClientEntityPart">
	</android-2_3:OrgApacheHttpClientEntity>
	<android-2_3:OrgApacheHttpClientParams rdf:about="&android-2_3;theOrgApacheHttpClientParamsPart">
	</android-2_3:OrgApacheHttpClientParams>
	<android-2_3:OrgApacheHttpClientProtocol rdf:about="&android-2_3;theOrgApacheHttpClientProtocolPart">
	</android-2_3:OrgApacheHttpClientProtocol>
	<android-2_3:OrgApacheHttpClientUtils rdf:about="&android-2_3;theOrgApacheHttpClientUtilsPart">
	</android-2_3:OrgApacheHttpClientUtils>
	<android-2_3:OrgApacheHttpParams rdf:about="&android-2_3;theOrgApacheHttpParamsPart">
	</android-2_3:OrgApacheHttpParams>
	<android-2_3:OrgApacheHttpConn rdf:about="&android-2_3;theOrgApacheHttpConnPart">
	</android-2_3:OrgApacheHttpConn>
	<android-2_3:OrgApacheHttpConnSsl rdf:about="&android-2_3;theOrgApacheHttpConnSslPart">
	</android-2_3:OrgApacheHttpConnSsl>
	<android-2_3:OrgApacheHttpConnRouting rdf:about="&android-2_3;theOrgApacheHttpConnRoutingPart">
	</android-2_3:OrgApacheHttpConnRouting>
	<android-2_3:OrgApacheHttpConnScheme rdf:about="&android-2_3;theOrgApacheHttpConnSchemePart">
	</android-2_3:OrgApacheHttpConnScheme>
	<android-2_3:OrgApacheHttpConnUtil rdf:about="&android-2_3;theOrgApacheHttpConnUtilPart">
	</android-2_3:OrgApacheHttpConnUtil>
	<android-2_3:OrgApacheHttpConnParams rdf:about="&android-2_3;theOrgApacheHttpConnParamsPart">
	</android-2_3:OrgApacheHttpConnParams>
	<android-2_3:OrgApacheHttpProtocol rdf:about="&android-2_3;theOrgApacheHttpProtocolPart">
	</android-2_3:OrgApacheHttpProtocol>
	<android-2_3:OrgApacheHttpEntity rdf:about="&android-2_3;theOrgApacheHttpEntityPart">
	</android-2_3:OrgApacheHttpEntity>
	<android-2_3:OrgApacheHttpImpl rdf:about="&android-2_3;theOrgApacheHttpImplPart">
	</android-2_3:OrgApacheHttpImpl>
	<android-2_3:OrgApacheHttpImplEntity rdf:about="&android-2_3;theOrgApacheHttpImplEntityPart">
	</android-2_3:OrgApacheHttpImplEntity>
	<android-2_3:OrgApacheHttpImplConn rdf:about="&android-2_3;theOrgApacheHttpImplConnPart">
	</android-2_3:OrgApacheHttpImplConn>
	<android-2_3:OrgApacheHttpImplConnTsccm rdf:about="&android-2_3;theOrgApacheHttpImplConnTsccmPart">
	</android-2_3:OrgApacheHttpImplConnTsccm>
	<android-2_3:OrgApacheHttpImplIo rdf:about="&android-2_3;theOrgApacheHttpImplIoPart">
	</android-2_3:OrgApacheHttpImplIo>
	<android-2_3:OrgApacheHttpImplCookie rdf:about="&android-2_3;theOrgApacheHttpImplCookiePart">
	</android-2_3:OrgApacheHttpImplCookie>
	<android-2_3:OrgApacheHttpImplAuth rdf:about="&android-2_3;theOrgApacheHttpImplAuthPart">
	</android-2_3:OrgApacheHttpImplAuth>
	<android-2_3:OrgApacheHttpImplClient rdf:about="&android-2_3;theOrgApacheHttpImplClientPart">
	</android-2_3:OrgApacheHttpImplClient>
	<android-2_3:OrgApacheHttpIo rdf:about="&android-2_3;theOrgApacheHttpIoPart">
	</android-2_3:OrgApacheHttpIo>
	<android-2_3:OrgApacheHttpUtil rdf:about="&android-2_3;theOrgApacheHttpUtilPart">
	</android-2_3:OrgApacheHttpUtil>
	<android-2_3:OrgApacheHttpMessage rdf:about="&android-2_3;theOrgApacheHttpMessagePart">
	</android-2_3:OrgApacheHttpMessage>
	<android-2_3:OrgApacheHttpCookie rdf:about="&android-2_3;theOrgApacheHttpCookiePart">
	</android-2_3:OrgApacheHttpCookie>
	<android-2_3:OrgApacheHttpCookieParams rdf:about="&android-2_3;theOrgApacheHttpCookieParamsPart">
	</android-2_3:OrgApacheHttpCookieParams>
	<android-2_3:OrgApacheHttpAuth rdf:about="&android-2_3;theOrgApacheHttpAuthPart">
	</android-2_3:OrgApacheHttpAuth>
	<android-2_3:OrgApacheHttpAuthParams rdf:about="&android-2_3;theOrgApacheHttpAuthParamsPart">
	</android-2_3:OrgApacheHttpAuthParams>
	<android-2_3:OrgApacheCommonsLogging rdf:about="&android-2_3;theOrgApacheCommonsLoggingPart">
	</android-2_3:OrgApacheCommonsLogging>
	<android-2_3:OrgJson rdf:about="&android-2_3;theOrgJsonPart">
	</android-2_3:OrgJson>
	<android-2_3:DalvikBytecode rdf:about="&android-2_3;theDalvikBytecodePart">
	</android-2_3:DalvikBytecode>
	<android-2_3:DalvikAnnotation rdf:about="&android-2_3;theDalvikAnnotationPart">
	</android-2_3:DalvikAnnotation>
	<android-2_3:DalvikSystem rdf:about="&android-2_3;theDalvikSystemPart">
	</android-2_3:DalvikSystem>
	<android-2_3:JunitRunner rdf:about="&android-2_3;theJunitRunnerPart">
	</android-2_3:JunitRunner>
	<android-2_3:JunitFramework rdf:about="&android-2_3;theJunitFrameworkPart">
	</android-2_3:JunitFramework>
	<android-2_3:Android rdf:about="&android-2_3;theAndroidPart">
	</android-2_3:Android>
	<android-2_3:AndroidContent rdf:about="&android-2_3;theAndroidContentPart">
	</android-2_3:AndroidContent>
	<android-2_3:AndroidContentPm rdf:about="&android-2_3;theAndroidContentPmPart">
	</android-2_3:AndroidContentPm>
	<android-2_3:AndroidContentRes rdf:about="&android-2_3;theAndroidContentResPart">
	</android-2_3:AndroidContentRes>
	<android-2_3:AndroidOs rdf:about="&android-2_3;theAndroidOsPart">
	</android-2_3:AndroidOs>
	<android-2_3:AndroidOsStorage rdf:about="&android-2_3;theAndroidOsStoragePart">
	</android-2_3:AndroidOsStorage>
	<android-2_3:AndroidAccounts rdf:about="&android-2_3;theAndroidAccountsPart">
	</android-2_3:AndroidAccounts>
	<android-2_3:AndroidNet rdf:about="&android-2_3;theAndroidNetPart">
	</android-2_3:AndroidNet>
	<android-2_3:AndroidNetHttp rdf:about="&android-2_3;theAndroidNetHttpPart">
	</android-2_3:AndroidNetHttp>
	<android-2_3:AndroidNetSip rdf:about="&android-2_3;theAndroidNetSipPart">
	</android-2_3:AndroidNetSip>
	<android-2_3:AndroidNetWifi rdf:about="&android-2_3;theAndroidNetWifiPart">
	</android-2_3:AndroidNetWifi>
	<android-2_3:AndroidDatabase rdf:about="&android-2_3;theAndroidDatabasePart">
	</android-2_3:AndroidDatabase>
	<android-2_3:AndroidDatabaseSqlite rdf:about="&android-2_3;theAndroidDatabaseSqlitePart">
	</android-2_3:AndroidDatabaseSqlite>
	<android-2_3:AndroidUtil rdf:about="&android-2_3;theAndroidUtilPart">
	</android-2_3:AndroidUtil>
	<android-2_3:AndroidGraphics rdf:about="&android-2_3;theAndroidGraphicsPart">
	</android-2_3:AndroidGraphics>
	<android-2_3:AndroidGraphicsDrawable rdf:about="&android-2_3;theAndroidGraphicsDrawablePart">
	</android-2_3:AndroidGraphicsDrawable>
	<android-2_3:AndroidGraphicsDrawableShapes rdf:about="&android-2_3;theAndroidGraphicsDrawableShapesPart">
	</android-2_3:AndroidGraphicsDrawableShapes>
	<android-2_3:AndroidView rdf:about="&android-2_3;theAndroidViewPart">
	</android-2_3:AndroidView>
	<android-2_3:AndroidViewAccessibility rdf:about="&android-2_3;theAndroidViewAccessibilityPart">
	</android-2_3:AndroidViewAccessibility>
	<android-2_3:AndroidViewInputmethod rdf:about="&android-2_3;theAndroidViewInputmethodPart">
	</android-2_3:AndroidViewInputmethod>
	<android-2_3:AndroidViewAnimation rdf:about="&android-2_3;theAndroidViewAnimationPart">
	</android-2_3:AndroidViewAnimation>
	<android-2_3:AndroidAccessibilityservice rdf:about="&android-2_3;theAndroidAccessibilityservicePart">
	</android-2_3:AndroidAccessibilityservice>
	<android-2_3:AndroidApp rdf:about="&android-2_3;theAndroidAppPart">
	</android-2_3:AndroidApp>
	<android-2_3:AndroidAppBackup rdf:about="&android-2_3;theAndroidAppBackupPart">
	</android-2_3:AndroidAppBackup>
	<android-2_3:AndroidAppAdmin rdf:about="&android-2_3;theAndroidAppAdminPart">
	</android-2_3:AndroidAppAdmin>
	<android-2_3:AndroidTelephony rdf:about="&android-2_3;theAndroidTelephonyPart">
	</android-2_3:AndroidTelephony>
	<android-2_3:AndroidTelephonyCdma rdf:about="&android-2_3;theAndroidTelephonyCdmaPart">
	</android-2_3:AndroidTelephonyCdma>
	<android-2_3:AndroidTelephonyGsm rdf:about="&android-2_3;theAndroidTelephonyGsmPart">
	</android-2_3:AndroidTelephonyGsm>
	<android-2_3:AndroidText rdf:about="&android-2_3;theAndroidTextPart">
	</android-2_3:AndroidText>
	<android-2_3:AndroidTextUtil rdf:about="&android-2_3;theAndroidTextUtilPart">
	</android-2_3:AndroidTextUtil>
	<android-2_3:AndroidTextFormat rdf:about="&android-2_3;theAndroidTextFormatPart">
	</android-2_3:AndroidTextFormat>
	<android-2_3:AndroidTextMethod rdf:about="&android-2_3;theAndroidTextMethodPart">
	</android-2_3:AndroidTextMethod>
	<android-2_3:AndroidTextStyle rdf:about="&android-2_3;theAndroidTextStylePart">
	</android-2_3:AndroidTextStyle>
	<android-2_3:AndroidGesture rdf:about="&android-2_3;theAndroidGesturePart">
	</android-2_3:AndroidGesture>
	<android-2_3:AndroidWidget rdf:about="&android-2_3;theAndroidWidgetPart">
	</android-2_3:AndroidWidget>
	<android-2_3:AndroidLocation rdf:about="&android-2_3;theAndroidLocationPart">
	</android-2_3:AndroidLocation>
	<android-2_3:AndroidHardware rdf:about="&android-2_3;theAndroidHardwarePart">
	</android-2_3:AndroidHardware>
	<android-2_3:AndroidWebkit rdf:about="&android-2_3;theAndroidWebkitPart">
	</android-2_3:AndroidWebkit>
	<android-2_3:AndroidTest rdf:about="&android-2_3;theAndroidTestPart">
	</android-2_3:AndroidTest>
	<android-2_3:AndroidTestMock rdf:about="&android-2_3;theAndroidTestMockPart">
	</android-2_3:AndroidTestMock>
	<android-2_3:AndroidTestSuitebuilder rdf:about="&android-2_3;theAndroidTestSuitebuilderPart">
	</android-2_3:AndroidTestSuitebuilder>
	<android-2_3:AndroidTestSuitebuilderAnnotation rdf:about="&android-2_3;theAndroidTestSuitebuilderAnnotationPart">
	</android-2_3:AndroidTestSuitebuilderAnnotation>
	<android-2_3:AndroidPreference rdf:about="&android-2_3;theAndroidPreferencePart">
	</android-2_3:AndroidPreference>
	<android-2_3:AndroidMedia rdf:about="&android-2_3;theAndroidMediaPart">
	</android-2_3:AndroidMedia>
	<android-2_3:AndroidMediaAudiofx rdf:about="&android-2_3;theAndroidMediaAudiofxPart">
	</android-2_3:AndroidMediaAudiofx>
	<android-2_3:AndroidInputmethodservice rdf:about="&android-2_3;theAndroidInputmethodservicePart">
	</android-2_3:AndroidInputmethodservice>
	<android-2_3:AndroidServiceWallpaper rdf:about="&android-2_3;theAndroidServiceWallpaperPart">
	</android-2_3:AndroidServiceWallpaper>
	<android-2_3:AndroidBluetooth rdf:about="&android-2_3;theAndroidBluetoothPart">
	</android-2_3:AndroidBluetooth>
	<android-2_3:AndroidNfc rdf:about="&android-2_3;theAndroidNfcPart">
	</android-2_3:AndroidNfc>
	<android-2_3:AndroidProvider rdf:about="&android-2_3;theAndroidProviderPart">
	</android-2_3:AndroidProvider>
	<android-2_3:AndroidSax rdf:about="&android-2_3;theAndroidSaxPart">
	</android-2_3:AndroidSax>
	<android-2_3:AndroidAppwidget rdf:about="&android-2_3;theAndroidAppwidgetPart">
	</android-2_3:AndroidAppwidget>
	<android-2_3:AndroidOpengl rdf:about="&android-2_3;theAndroidOpenglPart">
	</android-2_3:AndroidOpengl>
	<android-2_3:AndroidSpeech rdf:about="&android-2_3;theAndroidSpeechPart">
	</android-2_3:AndroidSpeech>
	<android-2_3:AndroidSpeechTts rdf:about="&android-2_3;theAndroidSpeechTtsPart">
	</android-2_3:AndroidSpeechTts>
	<owl:Class rdf:about="&android-2_3;JavaxXmlClassLibrary">
		<owl:equivalentClass rdf:resource="&java-se-6;JavaxXmlClassLibrary"/>
		<owl:equivalentClass rdf:resource="&android-2_2;JavaxXmlClassLibrary"/>
		<rdfs:subClassOf rdf:resource="&java;JavaClassLibrary"/>
		<rdfs:comment xml:lang="en">JavaLibrary implementing the javax.xml package for Android 2.3</rdfs:comment>
		<rdfs:comment xml:lang="OWLManchester">platform:implementsInterface some JavaxXmlAPI</rdfs:comment>
	</owl:Class>
	<owl:Class rdf:about="&android-2_3;JavaxXmlDatatypeClassLibrary">
		<owl:equivalentClass rdf:resource="&java-se-6;JavaxXmlDatatypeClassLibrary"/>
		<rdfs:subClassOf rdf:resource="&android-2_2;JavaxXmlDatatypeClassLibrary"/>
		<rdfs:comment xml:lang="en">JavaLibrary implementing the javax.xml.datatype package for Android 2.3</rdfs:comment>
		<rdfs:comment xml:lang="OWLManchester">platform:implementsInterface some JavaxXmlDatatypeAPI</rdfs:comment>
	</owl:Class>
	<owl:Class rdf:about="&android-2_3;JavaxXmlNamespaceClassLibrary">
		<owl:equivalentClass rdf:resource="&java-se-6;JavaxXmlNamespaceClassLibrary"/>
		<owl:equivalentClass rdf:resource="&android-2_2;JavaxXmlNamespaceClassLibrary"/>
		<rdfs:subClassOf rdf:resource="&java;JavaClassLibrary"/>
		<rdfs:comment xml:lang="en">JavaLibrary implementing the javax.xml.namespace package for Android 2.3</rdfs:comment>
		<rdfs:comment xml:lang="OWLManchester">platform:implementsInterface some JavaxXmlNamespaceAPI</rdfs:comment>
	</owl:Class>
	<owl:Class rdf:about="&android-2_3;JavaxXmlXpathClassLibrary">
		<owl:equivalentClass rdf:resource="&java-se-6;JavaxXmlXpathClassLibrary"/>
		<owl:equivalentClass rdf:resource="&android-2_2;JavaxXmlXpathClassLibrary"/>
		<rdfs:subClassOf rdf:resource="&java;JavaClassLibrary"/>
		<rdfs:comment xml:lang="en">JavaLibrary implementing the javax.xml.xpath package for Android 2.3</rdfs:comment>
		<rdfs:comment xml:lang="OWLManchester">platform:implementsInterface some JavaxXmlXpathAPI</rdfs:comment>
	</owl:Class>
	<owl:Class rdf:about="&android-2_3;JavaxXmlTransformClassLibrary">
		<owl:equivalentClass rdf:resource="&java-se-6;JavaxXmlTransformClassLibrary"/>
		<rdfs:subClassOf rdf:resource="&android-2_2;JavaxXmlTransformClassLibrary"/>
		<rdfs:comment xml:lang="en">JavaLibrary implementing the javax.xml.transform package for Android 2.3</rdfs:comment>
		<rdfs:comment xml:lang="OWLManchester">platform:implementsInterface some JavaxXmlTransformAPI</rdfs:comment>
	</owl:Class>
	<owl:Class rdf:about="&android-2_3;JavaxXmlTransformDomClassLibrary">
		<owl:equivalentClass rdf:resource="&java-se-6;JavaxXmlTransformDomClassLibrary"/>
		<owl:equivalentClass rdf:resource="&android-2_2;JavaxXmlTransformDomClassLibrary"/>
		<rdfs:subClassOf rdf:resource="&java;JavaClassLibrary"/>
		<rdfs:comment xml:lang="en">JavaLibrary implementing the javax.xml.transform.dom package for Android 2.3</rdfs:comment>
		<rdfs:comment xml:lang="OWLManchester">platform:implementsInterface some JavaxXmlTransformDomAPI</rdfs:comment>
	</owl:Class>
	<owl:Class rdf:about="&android-2_3;JavaxXmlTransformSaxClassLibrary">
		<owl:equivalentClass rdf:resource="&java-se-6;JavaxXmlTransformSaxClassLibrary"/>
		<rdfs:subClassOf rdf:resource="&android-2_2;JavaxXmlTransformSaxClassLibrary"/>
		<rdfs:comment xml:lang="en">JavaLibrary implementing the javax.xml.transform.sax package for Android 2.3</rdfs:comment>
		<rdfs:comment xml:lang="OWLManchester">platform:implementsInterface some JavaxXmlTransformSaxAPI</rdfs:comment>
	</owl:Class>
	<owl:Class rdf:about="&android-2_3;JavaxXmlTransformStreamClassLibrary">
		<owl:equivalentClass rdf:resource="&java-se-6;JavaxXmlTransformStreamClassLibrary"/>
		<owl:equivalentClass rdf:resource="&android-2_2;JavaxXmlTransformStreamClassLibrary"/>
		<rdfs:subClassOf rdf:resource="&java;JavaClassLibrary"/>
		<rdfs:comment xml:lang="en">JavaLibrary implementing the javax.xml.transform.stream package for Android 2.3</rdfs:comment>
		<rdfs:comment xml:lang="OWLManchester">platform:implementsInterface some JavaxXmlTransformStreamAPI</rdfs:comment>
	</owl:Class>
	<owl:Class rdf:about="&android-2_3;JavaxXmlParsersClassLibrary">
		<owl:equivalentClass rdf:resource="&java-se-6;JavaxXmlParsersClassLibrary"/>
		<rdfs:subClassOf rdf:resource="&android-2_2;JavaxXmlParsersClassLibrary"/>
		<rdfs:comment xml:lang="en">JavaLibrary implementing the javax.xml.parsers package for Android 2.3</rdfs:comment>
		<rdfs:comment xml:lang="OWLManchester">platform:implementsInterface some JavaxXmlParsersAPI</rdfs:comment>
	</owl:Class>
	<owl:Class rdf:about="&android-2_3;JavaxXmlValidationClassLibrary">
		<rdfs:subClassOf rdf:resource="&java-se-6;JavaxXmlValidationClassLibrary"/>
		<rdfs:subClassOf rdf:resource="&android-2_2;JavaxXmlValidationClassLibrary"/>
		<rdfs:comment xml:lang="en">JavaLibrary implementing the javax.xml.validation package for Android 2.3</rdfs:comment>
		<rdfs:comment xml:lang="OWLManchester">platform:implementsInterface some JavaxXmlValidationAPI</rdfs:comment>
	</owl:Class>
	<owl:Class rdf:about="&android-2_3;JavaxSecurityCertClassLibrary">
		<owl:equivalentClass rdf:resource="&java-se-6;JavaxSecurityCertClassLibrary"/>
		<owl:equivalentClass rdf:resource="&android-2_2;JavaxSecurityCertClassLibrary"/>
		<rdfs:subClassOf rdf:resource="&java;JavaClassLibrary"/>
		<rdfs:comment xml:lang="en">JavaLibrary implementing the javax.security.cert package for Android 2.3</rdfs:comment>
		<rdfs:comment xml:lang="OWLManchester">platform:implementsInterface some JavaxSecurityCertAPI</rdfs:comment>
	</owl:Class>
	<owl:Class rdf:about="&android-2_3;JavaxSecurityAuthClassLibrary">
		<owl:equivalentClass rdf:resource="&android-2_2;JavaxSecurityAuthClassLibrary"/>
		<rdfs:subClassOf rdf:resource="&java;JavaClassLibrary"/>
		<rdfs:comment xml:lang="en">JavaLibrary implementing the javax.security.auth package for Android 2.3</rdfs:comment>
		<rdfs:comment xml:lang="OWLManchester">platform:implementsInterface some JavaxSecurityAuthAPI</rdfs:comment>
	</owl:Class>
	<owl:Class rdf:about="&android-2_3;JavaxSecurityAuthCallbackClassLibrary">
		<owl:equivalentClass rdf:resource="&android-2_2;JavaxSecurityAuthCallbackClassLibrary"/>
		<rdfs:subClassOf rdf:resource="&java;JavaClassLibrary"/>
		<rdfs:comment xml:lang="en">JavaLibrary implementing the javax.security.auth.callback package for Android 2.3</rdfs:comment>
		<rdfs:comment xml:lang="OWLManchester">platform:implementsInterface some JavaxSecurityAuthCallbackAPI</rdfs:comment>
	</owl:Class>
	<owl:Class rdf:about="&android-2_3;JavaxSecurityAuthLoginClassLibrary">
		<owl:equivalentClass rdf:resource="&android-2_2;JavaxSecurityAuthLoginClassLibrary"/>
		<rdfs:subClassOf rdf:resource="&java;JavaClassLibrary"/>
		<rdfs:comment xml:lang="en">JavaLibrary implementing the javax.security.auth.login package for Android 2.3</rdfs:comment>
		<rdfs:comment xml:lang="OWLManchester">platform:implementsInterface some JavaxSecurityAuthLoginAPI</rdfs:comment>
	</owl:Class>
	<owl:Class rdf:about="&android-2_3;JavaxSecurityAuthX500ClassLibrary">
		<rdfs:subClassOf rdf:resource="&android-2_2;JavaxSecurityAuthX500ClassLibrary"/>
		<rdfs:comment xml:lang="en">JavaLibrary implementing the javax.security.auth.x500 package for Android 2.3</rdfs:comment>
		<rdfs:comment xml:lang="OWLManchester">platform:implementsInterface some JavaxSecurityAuthX500API</rdfs:comment>
	</owl:Class>
	<owl:Class rdf:about="&android-2_3;JavaxSqlClassLibrary">
		<rdfs:subClassOf rdf:resource="&android-2_2;JavaxSqlClassLibrary"/>
		<rdfs:comment xml:lang="en">JavaLibrary implementing the javax.sql package for Android 2.3</rdfs:comment>
		<rdfs:comment xml:lang="OWLManchester">platform:implementsInterface some JavaxSqlAPI</rdfs:comment>
	</owl:Class>
	<owl:Class rdf:about="&android-2_3;JavaxCryptoClassLibrary">
		<owl:equivalentClass rdf:resource="&java-se-6;JavaxCryptoClassLibrary"/>
		<owl:equivalentClass rdf:resource="&android-2_2;JavaxCryptoClassLibrary"/>
		<rdfs:subClassOf rdf:resource="&java;JavaClassLibrary"/>
		<rdfs:comment xml:lang="en">JavaLibrary implementing the javax.crypto package for Android 2.3</rdfs:comment>
		<rdfs:comment xml:lang="OWLManchester">platform:implementsInterface some JavaxCryptoAPI</rdfs:comment>
	</owl:Class>
	<owl:Class rdf:about="&android-2_3;JavaxCryptoInterfacesClassLibrary">
		<owl:equivalentClass rdf:resource="&java-se-6;JavaxCryptoInterfacesClassLibrary"/>
		<owl:equivalentClass rdf:resource="&android-2_2;JavaxCryptoInterfacesClassLibrary"/>
		<rdfs:subClassOf rdf:resource="&java;JavaClassLibrary"/>
		<rdfs:comment xml:lang="en">JavaLibrary implementing the javax.crypto.interfaces package for Android 2.3</rdfs:comment>
		<rdfs:comment xml:lang="OWLManchester">platform:implementsInterface some JavaxCryptoInterfacesAPI</rdfs:comment>
	</owl:Class>
	<owl:Class rdf:about="&android-2_3;JavaxCryptoSpecClassLibrary">
		<owl:equivalentClass rdf:resource="&java-se-6;JavaxCryptoSpecClassLibrary"/>
		<owl:equivalentClass rdf:resource="&android-2_2;JavaxCryptoSpecClassLibrary"/>
		<rdfs:subClassOf rdf:resource="&java;JavaClassLibrary"/>
		<rdfs:comment xml:lang="en">JavaLibrary implementing the javax.crypto.spec package for Android 2.3</rdfs:comment>
		<rdfs:comment xml:lang="OWLManchester">platform:implementsInterface some JavaxCryptoSpecAPI</rdfs:comment>
	</owl:Class>
	<owl:Class rdf:about="&android-2_3;JavaxMicroeditionKhronosEglClassLibrary">
		<owl:equivalentClass rdf:resource="&android-2_2;JavaxMicroeditionKhronosEglClassLibrary"/>
		<rdfs:subClassOf rdf:resource="&java;JavaClassLibrary"/>
		<rdfs:comment xml:lang="en">JavaLibrary implementing the javax.microedition.khronos.egl package for Android 2.3</rdfs:comment>
		<rdfs:comment xml:lang="OWLManchester">platform:implementsInterface some JavaxMicroeditionKhronosEglAPI</rdfs:comment>
	</owl:Class>
	<owl:Class rdf:about="&android-2_3;JavaxMicroeditionKhronosOpenglesClassLibrary">
		<owl:equivalentClass rdf:resource="&android-2_2;JavaxMicroeditionKhronosOpenglesClassLibrary"/>
		<rdfs:subClassOf rdf:resource="&java;JavaClassLibrary"/>
		<rdfs:comment xml:lang="en">JavaLibrary implementing the javax.microedition.khronos.opengles package for Android 2.3</rdfs:comment>
		<rdfs:comment xml:lang="OWLManchester">platform:implementsInterface some JavaxMicroeditionKhronosOpenglesAPI</rdfs:comment>
	</owl:Class>
	<owl:Class rdf:about="&android-2_3;JavaxNetClassLibrary">
		<owl:equivalentClass rdf:resource="&java-se-6;JavaxNetClassLibrary"/>
		<owl:equivalentClass rdf:resource="&android-2_2;JavaxNetClassLibrary"/>
		<rdfs:subClassOf rdf:resource="&java;JavaClassLibrary"/>
		<rdfs:comment xml:lang="en">JavaLibrary implementing the javax.net package for Android 2.3</rdfs:comment>
		<rdfs:comment xml:lang="OWLManchester">platform:implementsInterface some JavaxNetAPI</rdfs:comment>
	</owl:Class>
	<owl:Class rdf:about="&android-2_3;JavaxNetSslClassLibrary">
		<owl:equivalentClass rdf:resource="&java-se-6;JavaxNetSslClassLibrary"/>
		<rdfs:subClassOf rdf:resource="&android-2_2;JavaxNetSslClassLibrary"/>
		<rdfs:comment xml:lang="en">JavaLibrary implementing the javax.net.ssl package for Android 2.3</rdfs:comment>
		<rdfs:comment xml:lang="OWLManchester">platform:implementsInterface some JavaxNetSslAPI</rdfs:comment>
	</owl:Class>
	<owl:Class rdf:about="&android-2_3;JavaLangClassLibrary">
		<rdfs:subClassOf rdf:resource="&java;JavaClassLibrary"/>
		<rdfs:comment xml:lang="en">JavaLibrary implementing the java.lang package for Android 2.3</rdfs:comment>
		<rdfs:comment xml:lang="OWLManchester">platform:implementsInterface some JavaLangAPI</rdfs:comment>
	</owl:Class>
	<owl:Class rdf:about="&android-2_3;JavaLangReflectClassLibrary">
		<owl:equivalentClass rdf:resource="&java-se-6;JavaLangReflectClassLibrary"/>
		<owl:equivalentClass rdf:resource="&android-2_2;JavaLangReflectClassLibrary"/>
		<rdfs:subClassOf rdf:resource="&java;JavaClassLibrary"/>
		<rdfs:comment xml:lang="en">JavaLibrary implementing the java.lang.reflect package for Android 2.3</rdfs:comment>
		<rdfs:comment xml:lang="OWLManchester">platform:implementsInterface some JavaLangReflectAPI</rdfs:comment>
	</owl:Class>
	<owl:Class rdf:about="&android-2_3;JavaLangAnnotationClassLibrary">
		<owl:equivalentClass rdf:resource="&java-se-6;JavaLangAnnotationClassLibrary"/>
		<rdfs:subClassOf rdf:resource="&android-2_2;JavaLangAnnotationClassLibrary"/>
		<rdfs:comment xml:lang="en">JavaLibrary implementing the java.lang.annotation package for Android 2.3</rdfs:comment>
		<rdfs:comment xml:lang="OWLManchester">platform:implementsInterface some JavaLangAnnotationAPI</rdfs:comment>
	</owl:Class>
	<owl:Class rdf:about="&android-2_3;JavaLangRefClassLibrary">
		<owl:equivalentClass rdf:resource="&java-se-6;JavaLangRefClassLibrary"/>
		<owl:equivalentClass rdf:resource="&android-2_2;JavaLangRefClassLibrary"/>
		<rdfs:subClassOf rdf:resource="&java;JavaClassLibrary"/>
		<rdfs:comment xml:lang="en">JavaLibrary implementing the java.lang.ref package for Android 2.3</rdfs:comment>
		<rdfs:comment xml:lang="OWLManchester">platform:implementsInterface some JavaLangRefAPI</rdfs:comment>
	</owl:Class>
	<owl:Class rdf:about="&android-2_3;JavaUtilClassLibrary">
		<owl:equivalentClass rdf:resource="&java-se-6;JavaUtilClassLibrary"/>
		<rdfs:subClassOf rdf:resource="&android-2_2;JavaUtilClassLibrary"/>
		<rdfs:comment xml:lang="en">JavaLibrary implementing the java.util package for Android 2.3</rdfs:comment>
		<rdfs:comment xml:lang="OWLManchester">platform:implementsInterface some JavaUtilAPI</rdfs:comment>
	</owl:Class>
	<owl:Class rdf:about="&android-2_3;JavaUtilJarClassLibrary">
		<owl:equivalentClass rdf:resource="&java-se-6;JavaUtilJarClassLibrary"/>
		<owl:equivalentClass rdf:resource="&android-2_2;JavaUtilJarClassLibrary"/>
		<rdfs:subClassOf rdf:resource="&java;JavaClassLibrary"/>
		<rdfs:comment xml:lang="en">JavaLibrary implementing the java.util.jar package for Android 2.3</rdfs:comment>
		<rdfs:comment xml:lang="OWLManchester">platform:implementsInterface some JavaUtilJarAPI</rdfs:comment>
	</owl:Class>
	<owl:Class rdf:about="&android-2_3;JavaUtilZipClassLibrary">
		<owl:equivalentClass rdf:resource="&java-se-6;JavaUtilZipClassLibrary"/>
		<rdfs:subClassOf rdf:resource="&android-2_2;JavaUtilZipClassLibrary"/>
		<rdfs:comment xml:lang="en">JavaLibrary implementing the java.util.zip package for Android 2.3</rdfs:comment>
		<rdfs:comment xml:lang="OWLManchester">platform:implementsInterface some JavaUtilZipAPI</rdfs:comment>
	</owl:Class>
	<owl:Class rdf:about="&android-2_3;JavaUtilPrefsClassLibrary">
		<owl:equivalentClass rdf:resource="&java-se-6;JavaUtilPrefsClassLibrary"/>
		<owl:equivalentClass rdf:resource="&android-2_2;JavaUtilPrefsClassLibrary"/>
		<rdfs:subClassOf rdf:resource="&java;JavaClassLibrary"/>
		<rdfs:comment xml:lang="en">JavaLibrary implementing the java.util.prefs package for Android 2.3</rdfs:comment>
		<rdfs:comment xml:lang="OWLManchester">platform:implementsInterface some JavaUtilPrefsAPI</rdfs:comment>
	</owl:Class>
	<owl:Class rdf:about="&android-2_3;JavaUtilRegexClassLibrary">
		<owl:equivalentClass rdf:resource="&java-se-6;JavaUtilRegexClassLibrary"/>
		<owl:equivalentClass rdf:resource="&android-2_2;JavaUtilRegexClassLibrary"/>
		<rdfs:subClassOf rdf:resource="&java;JavaClassLibrary"/>
		<rdfs:comment xml:lang="en">JavaLibrary implementing the java.util.regex package for Android 2.3</rdfs:comment>
		<rdfs:comment xml:lang="OWLManchester">platform:implementsInterface some JavaUtilRegexAPI</rdfs:comment>
	</owl:Class>
	<owl:Class rdf:about="&android-2_3;JavaUtilConcurrentClassLibrary">
		<rdfs:subClassOf rdf:resource="&android-2_2;JavaUtilConcurrentClassLibrary"/>
		<rdfs:comment xml:lang="en">JavaLibrary implementing the java.util.concurrent package for Android 2.3</rdfs:comment>
		<rdfs:comment xml:lang="OWLManchester">platform:implementsInterface some JavaUtilConcurrentAPI</rdfs:comment>
	</owl:Class>
	<owl:Class rdf:about="&android-2_3;JavaUtilConcurrentAtomicClassLibrary">
		<owl:equivalentClass rdf:resource="&java-se-6;JavaUtilConcurrentAtomicClassLibrary"/>
		<rdfs:subClassOf rdf:resource="&android-2_2;JavaUtilConcurrentAtomicClassLibrary"/>
		<rdfs:comment xml:lang="en">JavaLibrary implementing the java.util.concurrent.atomic package for Android 2.3</rdfs:comment>
		<rdfs:comment xml:lang="OWLManchester">platform:implementsInterface some JavaUtilConcurrentAtomicAPI</rdfs:comment>
	</owl:Class>
	<owl:Class rdf:about="&android-2_3;JavaUtilConcurrentLocksClassLibrary">
		<owl:equivalentClass rdf:resource="&java-se-6;JavaUtilConcurrentLocksClassLibrary"/>
		<rdfs:subClassOf rdf:resource="&android-2_2;JavaUtilConcurrentLocksClassLibrary"/>
		<rdfs:comment xml:lang="en">JavaLibrary implementing the java.util.concurrent.locks package for Android 2.3</rdfs:comment>
		<rdfs:comment xml:lang="OWLManchester">platform:implementsInterface some JavaUtilConcurrentLocksAPI</rdfs:comment>
	</owl:Class>
	<owl:Class rdf:about="&android-2_3;JavaUtilLoggingClassLibrary">
		<owl:equivalentClass rdf:resource="&java-se-6;JavaUtilLoggingClassLibrary"/>
		<rdfs:subClassOf rdf:resource="&android-2_2;JavaUtilLoggingClassLibrary"/>
		<rdfs:comment xml:lang="en">JavaLibrary implementing the java.util.logging package for Android 2.3</rdfs:comment>
		<rdfs:comment xml:lang="OWLManchester">platform:implementsInterface some JavaUtilLoggingAPI</rdfs:comment>
	</owl:Class>
	<owl:Class rdf:about="&android-2_3;JavaMathClassLibrary">
		<owl:equivalentClass rdf:resource="&java-se-6;JavaMathClassLibrary"/>
		<rdfs:subClassOf rdf:resource="&android-2_2;JavaMathClassLibrary"/>
		<rdfs:comment xml:lang="en">JavaLibrary implementing the java.math package for Android 2.3</rdfs:comment>
		<rdfs:comment xml:lang="OWLManchester">platform:implementsInterface some JavaMathAPI</rdfs:comment>
	</owl:Class>
	<owl:Class rdf:about="&android-2_3;JavaIoClassLibrary">
		<owl:equivalentClass rdf:resource="&java-se-6;JavaIoClassLibrary"/>
		<rdfs:subClassOf rdf:resource="&android-2_2;JavaIoClassLibrary"/>
		<rdfs:comment xml:lang="en">JavaLibrary implementing the java.io package for Android 2.3</rdfs:comment>
		<rdfs:comment xml:lang="OWLManchester">platform:implementsInterface some JavaIoAPI</rdfs:comment>
	</owl:Class>
	<owl:Class rdf:about="&android-2_3;JavaNetClassLibrary">
		<owl:equivalentClass rdf:resource="&java-se-6;JavaNetClassLibrary"/>
		<rdfs:subClassOf rdf:resource="&android-2_2;JavaNetClassLibrary"/>
		<rdfs:comment xml:lang="en">JavaLibrary implementing the java.net package for Android 2.3</rdfs:comment>
		<rdfs:comment xml:lang="OWLManchester">platform:implementsInterface some JavaNetAPI</rdfs:comment>
	</owl:Class>
	<owl:Class rdf:about="&android-2_3;JavaSecurityClassLibrary">
		<rdfs:subClassOf rdf:resource="&android-2_2;JavaSecurityClassLibrary"/>
		<rdfs:comment xml:lang="en">JavaLibrary implementing the java.security package for Android 2.3</rdfs:comment>
		<rdfs:comment xml:lang="OWLManchester">platform:implementsInterface some JavaSecurityAPI</rdfs:comment>
	</owl:Class>
	<owl:Class rdf:about="&android-2_3;JavaSecuritySpecClassLibrary">
		<owl:equivalentClass rdf:resource="&java-se-6;JavaSecuritySpecClassLibrary"/>
		<owl:equivalentClass rdf:resource="&android-2_2;JavaSecuritySpecClassLibrary"/>
		<rdfs:subClassOf rdf:resource="&java;JavaClassLibrary"/>
		<rdfs:comment xml:lang="en">JavaLibrary implementing the java.security.spec package for Android 2.3</rdfs:comment>
		<rdfs:comment xml:lang="OWLManchester">platform:implementsInterface some JavaSecuritySpecAPI</rdfs:comment>
	</owl:Class>
	<owl:Class rdf:about="&android-2_3;JavaSecurityCertClassLibrary">
		<owl:equivalentClass rdf:resource="&java-se-6;JavaSecurityCertClassLibrary"/>
		<owl:equivalentClass rdf:resource="&android-2_2;JavaSecurityCertClassLibrary"/>
		<rdfs:subClassOf rdf:resource="&java;JavaClassLibrary"/>
		<rdfs:comment xml:lang="en">JavaLibrary implementing the java.security.cert package for Android 2.3</rdfs:comment>
		<rdfs:comment xml:lang="OWLManchester">platform:implementsInterface some JavaSecurityCertAPI</rdfs:comment>
	</owl:Class>
	<owl:Class rdf:about="&android-2_3;JavaSecurityInterfacesClassLibrary">
		<owl:equivalentClass rdf:resource="&java-se-6;JavaSecurityInterfacesClassLibrary"/>
		<owl:equivalentClass rdf:resource="&android-2_2;JavaSecurityInterfacesClassLibrary"/>
		<rdfs:subClassOf rdf:resource="&java;JavaClassLibrary"/>
		<rdfs:comment xml:lang="en">JavaLibrary implementing the java.security.interfaces package for Android 2.3</rdfs:comment>
		<rdfs:comment xml:lang="OWLManchester">platform:implementsInterface some JavaSecurityInterfacesAPI</rdfs:comment>
	</owl:Class>
	<owl:Class rdf:about="&android-2_3;JavaSecurityAclClassLibrary">
		<owl:equivalentClass rdf:resource="&java-se-6;JavaSecurityAclClassLibrary"/>
		<owl:equivalentClass rdf:resource="&android-2_2;JavaSecurityAclClassLibrary"/>
		<rdfs:subClassOf rdf:resource="&java;JavaClassLibrary"/>
		<rdfs:comment xml:lang="en">JavaLibrary implementing the java.security.acl package for Android 2.3</rdfs:comment>
		<rdfs:comment xml:lang="OWLManchester">platform:implementsInterface some JavaSecurityAclAPI</rdfs:comment>
	</owl:Class>
	<owl:Class rdf:about="&android-2_3;JavaSqlClassLibrary">
		<owl:equivalentClass rdf:resource="&java-se-6;JavaSqlClassLibrary"/>
		<rdfs:subClassOf rdf:resource="&android-2_2;JavaSqlClassLibrary"/>
		<rdfs:comment xml:lang="en">JavaLibrary implementing the java.sql package for Android 2.3</rdfs:comment>
		<rdfs:comment xml:lang="OWLManchester">platform:implementsInterface some JavaSqlAPI</rdfs:comment>
	</owl:Class>
	<owl:Class rdf:about="&android-2_3;JavaNioClassLibrary">
		<owl:equivalentClass rdf:resource="&java-se-6;JavaNioClassLibrary"/>
		<rdfs:subClassOf rdf:resource="&android-2_2;JavaNioClassLibrary"/>
		<rdfs:comment xml:lang="en">JavaLibrary implementing the java.nio package for Android 2.3</rdfs:comment>
		<rdfs:comment xml:lang="OWLManchester">platform:implementsInterface some JavaNioAPI</rdfs:comment>
	</owl:Class>
	<owl:Class rdf:about="&android-2_3;JavaNioChannelsClassLibrary">
		<owl:equivalentClass rdf:resource="&java-se-6;JavaNioChannelsClassLibrary"/>
		<owl:equivalentClass rdf:resource="&android-2_2;JavaNioChannelsClassLibrary"/>
		<rdfs:subClassOf rdf:resource="&java;JavaClassLibrary"/>
		<rdfs:comment xml:lang="en">JavaLibrary implementing the java.nio.channels package for Android 2.3</rdfs:comment>
		<rdfs:comment xml:lang="OWLManchester">platform:implementsInterface some JavaNioChannelsAPI</rdfs:comment>
	</owl:Class>
	<owl:Class rdf:about="&android-2_3;JavaNioChannelsSpiClassLibrary">
		<owl:equivalentClass rdf:resource="&java-se-6;JavaNioChannelsSpiClassLibrary"/>
		<owl:equivalentClass rdf:resource="&android-2_2;JavaNioChannelsSpiClassLibrary"/>
		<rdfs:subClassOf rdf:resource="&java;JavaClassLibrary"/>
		<rdfs:comment xml:lang="en">JavaLibrary implementing the java.nio.channels.spi package for Android 2.3</rdfs:comment>
		<rdfs:comment xml:lang="OWLManchester">platform:implementsInterface some JavaNioChannelsSpiAPI</rdfs:comment>
	</owl:Class>
	<owl:Class rdf:about="&android-2_3;JavaNioCharsetClassLibrary">
		<owl:equivalentClass rdf:resource="&java-se-6;JavaNioCharsetClassLibrary"/>
		<owl:equivalentClass rdf:resource="&android-2_2;JavaNioCharsetClassLibrary"/>
		<rdfs:subClassOf rdf:resource="&java;JavaClassLibrary"/>
		<rdfs:comment xml:lang="en">JavaLibrary implementing the java.nio.charset package for Android 2.3</rdfs:comment>
		<rdfs:comment xml:lang="OWLManchester">platform:implementsInterface some JavaNioCharsetAPI</rdfs:comment>
	</owl:Class>
	<owl:Class rdf:about="&android-2_3;JavaNioCharsetSpiClassLibrary">
		<owl:equivalentClass rdf:resource="&java-se-6;JavaNioCharsetSpiClassLibrary"/>
		<owl:equivalentClass rdf:resource="&android-2_2;JavaNioCharsetSpiClassLibrary"/>
		<rdfs:subClassOf rdf:resource="&java;JavaClassLibrary"/>
		<rdfs:comment xml:lang="en">JavaLibrary implementing the java.nio.charset.spi package for Android 2.3</rdfs:comment>
		<rdfs:comment xml:lang="OWLManchester">platform:implementsInterface some JavaNioCharsetSpiAPI</rdfs:comment>
	</owl:Class>
	<owl:Class rdf:about="&android-2_3;JavaBeansClassLibrary">
		<owl:equivalentClass rdf:resource="&android-2_2;JavaBeansClassLibrary"/>
		<rdfs:subClassOf rdf:resource="&java;JavaClassLibrary"/>
		<rdfs:comment xml:lang="en">JavaLibrary implementing the java.beans package for Android 2.3</rdfs:comment>
		<rdfs:comment xml:lang="OWLManchester">platform:implementsInterface some JavaBeansAPI</rdfs:comment>
	</owl:Class>
	<owl:Class rdf:about="&android-2_3;JavaTextClassLibrary">
		<rdfs:subClassOf rdf:resource="&java-se-6;JavaTextClassLibrary"/>
		<rdfs:comment xml:lang="en">JavaLibrary implementing the java.text package for Android 2.3</rdfs:comment>
		<rdfs:comment xml:lang="OWLManchester">platform:implementsInterface some JavaTextAPI</rdfs:comment>
	</owl:Class>
	<owl:Class rdf:about="&android-2_3;JavaAwtFontClassLibrary">
		<rdfs:subClassOf rdf:resource="&android-2_2;JavaAwtFontClassLibrary"/>
		<rdfs:comment xml:lang="en">JavaLibrary implementing the java.awt.font package for Android 2.3</rdfs:comment>
		<rdfs:comment xml:lang="OWLManchester">platform:implementsInterface some JavaAwtFontAPI</rdfs:comment>
	</owl:Class>
	<owl:Class rdf:about="&android-2_3;OrgXmlSaxClassLibrary">
		<owl:equivalentClass rdf:resource="&java-se-6;OrgXmlSaxClassLibrary"/>
		<owl:equivalentClass rdf:resource="&android-2_2;OrgXmlSaxClassLibrary"/>
		<rdfs:subClassOf rdf:resource="&java;JavaClassLibrary"/>
		<rdfs:comment xml:lang="en">JavaLibrary implementing the org.xml.sax package for Android 2.3</rdfs:comment>
		<rdfs:comment xml:lang="OWLManchester">platform:implementsInterface some OrgXmlSaxAPI</rdfs:comment>
	</owl:Class>
	<owl:Class rdf:about="&android-2_3;OrgXmlSaxExtClassLibrary">
		<owl:equivalentClass rdf:resource="&java-se-6;OrgXmlSaxExtClassLibrary"/>
		<owl:equivalentClass rdf:resource="&android-2_2;OrgXmlSaxExtClassLibrary"/>
		<rdfs:subClassOf rdf:resource="&java;JavaClassLibrary"/>
		<rdfs:comment xml:lang="en">JavaLibrary implementing the org.xml.sax.ext package for Android 2.3</rdfs:comment>
		<rdfs:comment xml:lang="OWLManchester">platform:implementsInterface some OrgXmlSaxExtAPI</rdfs:comment>
	</owl:Class>
	<owl:Class rdf:about="&android-2_3;OrgXmlSaxHelpersClassLibrary">
		<owl:equivalentClass rdf:resource="&java-se-6;OrgXmlSaxHelpersClassLibrary"/>
		<owl:equivalentClass rdf:resource="&android-2_2;OrgXmlSaxHelpersClassLibrary"/>
		<rdfs:subClassOf rdf:resource="&java;JavaClassLibrary"/>
		<rdfs:comment xml:lang="en">JavaLibrary implementing the org.xml.sax.helpers package for Android 2.3</rdfs:comment>
		<rdfs:comment xml:lang="OWLManchester">platform:implementsInterface some OrgXmlSaxHelpersAPI</rdfs:comment>
	</owl:Class>
	<owl:Class rdf:about="&android-2_3;OrgW3cDomClassLibrary">
		<owl:equivalentClass rdf:resource="&java-se-6;OrgW3cDomClassLibrary"/>
		<owl:equivalentClass rdf:resource="&android-2_2;OrgW3cDomClassLibrary"/>
		<rdfs:subClassOf rdf:resource="&java;JavaClassLibrary"/>
		<rdfs:comment xml:lang="en">JavaLibrary implementing the org.w3c.dom package for Android 2.3</rdfs:comment>
		<rdfs:comment xml:lang="OWLManchester">platform:implementsInterface some OrgW3cDomAPI</rdfs:comment>
	</owl:Class>
	<owl:Class rdf:about="&android-2_3;OrgW3cDomLsClassLibrary">
		<owl:equivalentClass rdf:resource="&android-2_2;OrgW3cDomLsClassLibrary"/>
		<rdfs:subClassOf rdf:resource="&java;JavaClassLibrary"/>
		<rdfs:comment xml:lang="en">JavaLibrary implementing the org.w3c.dom.ls package for Android 2.3</rdfs:comment>
		<rdfs:comment xml:lang="OWLManchester">platform:implementsInterface some OrgW3cDomLsAPI</rdfs:comment>
	</owl:Class>
	<owl:Class rdf:about="&android-2_3;OrgXmlpullV1ClassLibrary">
		<owl:equivalentClass rdf:resource="&android-2_2;OrgXmlpullV1ClassLibrary"/>
		<rdfs:subClassOf rdf:resource="&java;JavaClassLibrary"/>
		<rdfs:comment xml:lang="en">JavaLibrary implementing the org.xmlpull.v1 package for Android 2.3</rdfs:comment>
		<rdfs:comment xml:lang="OWLManchester">platform:implementsInterface some OrgXmlpullV1API</rdfs:comment>
	</owl:Class>
	<owl:Class rdf:about="&android-2_3;OrgXmlpullV1Sax2ClassLibrary">
		<owl:equivalentClass rdf:resource="&android-2_2;OrgXmlpullV1Sax2ClassLibrary"/>
		<rdfs:subClassOf rdf:resource="&java;JavaClassLibrary"/>
		<rdfs:comment xml:lang="en">JavaLibrary implementing the org.xmlpull.v1.sax2 package for Android 2.3</rdfs:comment>
		<rdfs:comment xml:lang="OWLManchester">platform:implementsInterface some OrgXmlpullV1Sax2API</rdfs:comment>
	</owl:Class>
	<owl:Class rdf:about="&android-2_3;OrgApacheHttpClassLibrary">
		<owl:equivalentClass rdf:resource="&android-2_2;OrgApacheHttpClassLibrary"/>
		<rdfs:subClassOf rdf:resource="&java;JavaClassLibrary"/>
		<rdfs:comment xml:lang="en">JavaLibrary implementing the org.apache.http package for Android 2.3</rdfs:comment>
		<rdfs:comment xml:lang="OWLManchester">platform:implementsInterface some OrgApacheHttpAPI</rdfs:comment>
	</owl:Class>
	<owl:Class rdf:about="&android-2_3;OrgApacheHttpClientClassLibrary">
		<owl:equivalentClass rdf:resource="&android-2_2;OrgApacheHttpClientClassLibrary"/>
		<rdfs:subClassOf rdf:resource="&java;JavaClassLibrary"/>
		<rdfs:comment xml:lang="en">JavaLibrary implementing the org.apache.http.client package for Android 2.3</rdfs:comment>
		<rdfs:comment xml:lang="OWLManchester">platform:implementsInterface some OrgApacheHttpClientAPI</rdfs:comment>
	</owl:Class>
	<owl:Class rdf:about="&android-2_3;OrgApacheHttpClientMethodsClassLibrary">
		<owl:equivalentClass rdf:resource="&android-2_2;OrgApacheHttpClientMethodsClassLibrary"/>
		<rdfs:subClassOf rdf:resource="&java;JavaClassLibrary"/>
		<rdfs:comment xml:lang="en">JavaLibrary implementing the org.apache.http.client.methods package for Android 2.3</rdfs:comment>
		<rdfs:comment xml:lang="OWLManchester">platform:implementsInterface some OrgApacheHttpClientMethodsAPI</rdfs:comment>
	</owl:Class>
	<owl:Class rdf:about="&android-2_3;OrgApacheHttpClientEntityClassLibrary">
		<owl:equivalentClass rdf:resource="&android-2_2;OrgApacheHttpClientEntityClassLibrary"/>
		<rdfs:subClassOf rdf:resource="&java;JavaClassLibrary"/>
		<rdfs:comment xml:lang="en">JavaLibrary implementing the org.apache.http.client.entity package for Android 2.3</rdfs:comment>
		<rdfs:comment xml:lang="OWLManchester">platform:implementsInterface some OrgApacheHttpClientEntityAPI</rdfs:comment>
	</owl:Class>
	<owl:Class rdf:about="&android-2_3;OrgApacheHttpClientParamsClassLibrary">
		<owl:equivalentClass rdf:resource="&android-2_2;OrgApacheHttpClientParamsClassLibrary"/>
		<rdfs:subClassOf rdf:resource="&java;JavaClassLibrary"/>
		<rdfs:comment xml:lang="en">JavaLibrary implementing the org.apache.http.client.params package for Android 2.3</rdfs:comment>
		<rdfs:comment xml:lang="OWLManchester">platform:implementsInterface some OrgApacheHttpClientParamsAPI</rdfs:comment>
	</owl:Class>
	<owl:Class rdf:about="&android-2_3;OrgApacheHttpClientProtocolClassLibrary">
		<owl:equivalentClass rdf:resource="&android-2_2;OrgApacheHttpClientProtocolClassLibrary"/>
		<rdfs:subClassOf rdf:resource="&java;JavaClassLibrary"/>
		<rdfs:comment xml:lang="en">JavaLibrary implementing the org.apache.http.client.protocol package for Android 2.3</rdfs:comment>
		<rdfs:comment xml:lang="OWLManchester">platform:implementsInterface some OrgApacheHttpClientProtocolAPI</rdfs:comment>
	</owl:Class>
	<owl:Class rdf:about="&android-2_3;OrgApacheHttpClientUtilsClassLibrary">
		<owl:equivalentClass rdf:resource="&android-2_2;OrgApacheHttpClientUtilsClassLibrary"/>
		<rdfs:subClassOf rdf:resource="&java;JavaClassLibrary"/>
		<rdfs:comment xml:lang="en">JavaLibrary implementing the org.apache.http.client.utils package for Android 2.3</rdfs:comment>
		<rdfs:comment xml:lang="OWLManchester">platform:implementsInterface some OrgApacheHttpClientUtilsAPI</rdfs:comment>
	</owl:Class>
	<owl:Class rdf:about="&android-2_3;OrgApacheHttpParamsClassLibrary">
		<owl:equivalentClass rdf:resource="&android-2_2;OrgApacheHttpParamsClassLibrary"/>
		<rdfs:subClassOf rdf:resource="&java;JavaClassLibrary"/>
		<rdfs:comment xml:lang="en">JavaLibrary implementing the org.apache.http.params package for Android 2.3</rdfs:comment>
		<rdfs:comment xml:lang="OWLManchester">platform:implementsInterface some OrgApacheHttpParamsAPI</rdfs:comment>
	</owl:Class>
	<owl:Class rdf:about="&android-2_3;OrgApacheHttpConnClassLibrary">
		<owl:equivalentClass rdf:resource="&android-2_2;OrgApacheHttpConnClassLibrary"/>
		<rdfs:subClassOf rdf:resource="&java;JavaClassLibrary"/>
		<rdfs:comment xml:lang="en">JavaLibrary implementing the org.apache.http.conn package for Android 2.3</rdfs:comment>
		<rdfs:comment xml:lang="OWLManchester">platform:implementsInterface some OrgApacheHttpConnAPI</rdfs:comment>
	</owl:Class>
	<owl:Class rdf:about="&android-2_3;OrgApacheHttpConnSslClassLibrary">
		<owl:equivalentClass rdf:resource="&android-2_2;OrgApacheHttpConnSslClassLibrary"/>
		<rdfs:subClassOf rdf:resource="&java;JavaClassLibrary"/>
		<rdfs:comment xml:lang="en">JavaLibrary implementing the org.apache.http.conn.ssl package for Android 2.3</rdfs:comment>
		<rdfs:comment xml:lang="OWLManchester">platform:implementsInterface some OrgApacheHttpConnSslAPI</rdfs:comment>
	</owl:Class>
	<owl:Class rdf:about="&android-2_3;OrgApacheHttpConnRoutingClassLibrary">
		<rdfs:subClassOf rdf:resource="&android-2_2;OrgApacheHttpConnRoutingClassLibrary"/>
		<rdfs:comment xml:lang="en">JavaLibrary implementing the org.apache.http.conn.routing package for Android 2.3</rdfs:comment>
		<rdfs:comment xml:lang="OWLManchester">platform:implementsInterface some OrgApacheHttpConnRoutingAPI</rdfs:comment>
	</owl:Class>
	<owl:Class rdf:about="&android-2_3;OrgApacheHttpConnSchemeClassLibrary">
		<owl:equivalentClass rdf:resource="&android-2_2;OrgApacheHttpConnSchemeClassLibrary"/>
		<rdfs:subClassOf rdf:resource="&java;JavaClassLibrary"/>
		<rdfs:comment xml:lang="en">JavaLibrary implementing the org.apache.http.conn.scheme package for Android 2.3</rdfs:comment>
		<rdfs:comment xml:lang="OWLManchester">platform:implementsInterface some OrgApacheHttpConnSchemeAPI</rdfs:comment>
	</owl:Class>
	<owl:Class rdf:about="&android-2_3;OrgApacheHttpConnUtilClassLibrary">
		<owl:equivalentClass rdf:resource="&android-2_2;OrgApacheHttpConnUtilClassLibrary"/>
		<rdfs:subClassOf rdf:resource="&java;JavaClassLibrary"/>
		<rdfs:comment xml:lang="en">JavaLibrary implementing the org.apache.http.conn.util package for Android 2.3</rdfs:comment>
		<rdfs:comment xml:lang="OWLManchester">platform:implementsInterface some OrgApacheHttpConnUtilAPI</rdfs:comment>
	</owl:Class>
	<owl:Class rdf:about="&android-2_3;OrgApacheHttpConnParamsClassLibrary">
		<owl:equivalentClass rdf:resource="&android-2_2;OrgApacheHttpConnParamsClassLibrary"/>
		<rdfs:subClassOf rdf:resource="&java;JavaClassLibrary"/>
		<rdfs:comment xml:lang="en">JavaLibrary implementing the org.apache.http.conn.params package for Android 2.3</rdfs:comment>
		<rdfs:comment xml:lang="OWLManchester">platform:implementsInterface some OrgApacheHttpConnParamsAPI</rdfs:comment>
	</owl:Class>
	<owl:Class rdf:about="&android-2_3;OrgApacheHttpProtocolClassLibrary">
		<owl:equivalentClass rdf:resource="&android-2_2;OrgApacheHttpProtocolClassLibrary"/>
		<rdfs:subClassOf rdf:resource="&java;JavaClassLibrary"/>
		<rdfs:comment xml:lang="en">JavaLibrary implementing the org.apache.http.protocol package for Android 2.3</rdfs:comment>
		<rdfs:comment xml:lang="OWLManchester">platform:implementsInterface some OrgApacheHttpProtocolAPI</rdfs:comment>
	</owl:Class>
	<owl:Class rdf:about="&android-2_3;OrgApacheHttpEntityClassLibrary">
		<owl:equivalentClass rdf:resource="&android-2_2;OrgApacheHttpEntityClassLibrary"/>
		<rdfs:subClassOf rdf:resource="&java;JavaClassLibrary"/>
		<rdfs:comment xml:lang="en">JavaLibrary implementing the org.apache.http.entity package for Android 2.3</rdfs:comment>
		<rdfs:comment xml:lang="OWLManchester">platform:implementsInterface some OrgApacheHttpEntityAPI</rdfs:comment>
	</owl:Class>
	<owl:Class rdf:about="&android-2_3;OrgApacheHttpImplClassLibrary">
		<owl:equivalentClass rdf:resource="&android-2_2;OrgApacheHttpImplClassLibrary"/>
		<rdfs:subClassOf rdf:resource="&java;JavaClassLibrary"/>
		<rdfs:comment xml:lang="en">JavaLibrary implementing the org.apache.http.impl package for Android 2.3</rdfs:comment>
		<rdfs:comment xml:lang="OWLManchester">platform:implementsInterface some OrgApacheHttpImplAPI</rdfs:comment>
	</owl:Class>
	<owl:Class rdf:about="&android-2_3;OrgApacheHttpImplEntityClassLibrary">
		<owl:equivalentClass rdf:resource="&android-2_2;OrgApacheHttpImplEntityClassLibrary"/>
		<rdfs:subClassOf rdf:resource="&java;JavaClassLibrary"/>
		<rdfs:comment xml:lang="en">JavaLibrary implementing the org.apache.http.impl.entity package for Android 2.3</rdfs:comment>
		<rdfs:comment xml:lang="OWLManchester">platform:implementsInterface some OrgApacheHttpImplEntityAPI</rdfs:comment>
	</owl:Class>
	<owl:Class rdf:about="&android-2_3;OrgApacheHttpImplConnClassLibrary">
		<owl:equivalentClass rdf:resource="&android-2_2;OrgApacheHttpImplConnClassLibrary"/>
		<rdfs:subClassOf rdf:resource="&java;JavaClassLibrary"/>
		<rdfs:comment xml:lang="en">JavaLibrary implementing the org.apache.http.impl.conn package for Android 2.3</rdfs:comment>
		<rdfs:comment xml:lang="OWLManchester">platform:implementsInterface some OrgApacheHttpImplConnAPI</rdfs:comment>
	</owl:Class>
	<owl:Class rdf:about="&android-2_3;OrgApacheHttpImplConnTsccmClassLibrary">
		<owl:equivalentClass rdf:resource="&android-2_2;OrgApacheHttpImplConnTsccmClassLibrary"/>
		<rdfs:subClassOf rdf:resource="&java;JavaClassLibrary"/>
		<rdfs:comment xml:lang="en">JavaLibrary implementing the org.apache.http.impl.conn.tsccm package for Android 2.3</rdfs:comment>
		<rdfs:comment xml:lang="OWLManchester">platform:implementsInterface some OrgApacheHttpImplConnTsccmAPI</rdfs:comment>
	</owl:Class>
	<owl:Class rdf:about="&android-2_3;OrgApacheHttpImplIoClassLibrary">
		<owl:equivalentClass rdf:resource="&android-2_2;OrgApacheHttpImplIoClassLibrary"/>
		<rdfs:subClassOf rdf:resource="&java;JavaClassLibrary"/>
		<rdfs:comment xml:lang="en">JavaLibrary implementing the org.apache.http.impl.io package for Android 2.3</rdfs:comment>
		<rdfs:comment xml:lang="OWLManchester">platform:implementsInterface some OrgApacheHttpImplIoAPI</rdfs:comment>
	</owl:Class>
	<owl:Class rdf:about="&android-2_3;OrgApacheHttpImplCookieClassLibrary">
		<owl:equivalentClass rdf:resource="&android-2_2;OrgApacheHttpImplCookieClassLibrary"/>
		<rdfs:subClassOf rdf:resource="&java;JavaClassLibrary"/>
		<rdfs:comment xml:lang="en">JavaLibrary implementing the org.apache.http.impl.cookie package for Android 2.3</rdfs:comment>
		<rdfs:comment xml:lang="OWLManchester">platform:implementsInterface some OrgApacheHttpImplCookieAPI</rdfs:comment>
	</owl:Class>
	<owl:Class rdf:about="&android-2_3;OrgApacheHttpImplAuthClassLibrary">
		<owl:equivalentClass rdf:resource="&android-2_2;OrgApacheHttpImplAuthClassLibrary"/>
		<rdfs:subClassOf rdf:resource="&java;JavaClassLibrary"/>
		<rdfs:comment xml:lang="en">JavaLibrary implementing the org.apache.http.impl.auth package for Android 2.3</rdfs:comment>
		<rdfs:comment xml:lang="OWLManchester">platform:implementsInterface some OrgApacheHttpImplAuthAPI</rdfs:comment>
	</owl:Class>
	<owl:Class rdf:about="&android-2_3;OrgApacheHttpImplClientClassLibrary">
		<owl:equivalentClass rdf:resource="&android-2_2;OrgApacheHttpImplClientClassLibrary"/>
		<rdfs:subClassOf rdf:resource="&java;JavaClassLibrary"/>
		<rdfs:comment xml:lang="en">JavaLibrary implementing the org.apache.http.impl.client package for Android 2.3</rdfs:comment>
		<rdfs:comment xml:lang="OWLManchester">platform:implementsInterface some OrgApacheHttpImplClientAPI</rdfs:comment>
	</owl:Class>
	<owl:Class rdf:about="&android-2_3;OrgApacheHttpIoClassLibrary">
		<owl:equivalentClass rdf:resource="&android-2_2;OrgApacheHttpIoClassLibrary"/>
		<rdfs:subClassOf rdf:resource="&java;JavaClassLibrary"/>
		<rdfs:comment xml:lang="en">JavaLibrary implementing the org.apache.http.io package for Android 2.3</rdfs:comment>
		<rdfs:comment xml:lang="OWLManchester">platform:implementsInterface some OrgApacheHttpIoAPI</rdfs:comment>
	</owl:Class>
	<owl:Class rdf:about="&android-2_3;OrgApacheHttpUtilClassLibrary">
		<owl:equivalentClass rdf:resource="&android-2_2;OrgApacheHttpUtilClassLibrary"/>
		<rdfs:subClassOf rdf:resource="&java;JavaClassLibrary"/>
		<rdfs:comment xml:lang="en">JavaLibrary implementing the org.apache.http.util package for Android 2.3</rdfs:comment>
		<rdfs:comment xml:lang="OWLManchester">platform:implementsInterface some OrgApacheHttpUtilAPI</rdfs:comment>
	</owl:Class>
	<owl:Class rdf:about="&android-2_3;OrgApacheHttpMessageClassLibrary">
		<owl:equivalentClass rdf:resource="&android-2_2;OrgApacheHttpMessageClassLibrary"/>
		<rdfs:subClassOf rdf:resource="&java;JavaClassLibrary"/>
		<rdfs:comment xml:lang="en">JavaLibrary implementing the org.apache.http.message package for Android 2.3</rdfs:comment>
		<rdfs:comment xml:lang="OWLManchester">platform:implementsInterface some OrgApacheHttpMessageAPI</rdfs:comment>
	</owl:Class>
	<owl:Class rdf:about="&android-2_3;OrgApacheHttpCookieClassLibrary">
		<owl:equivalentClass rdf:resource="&android-2_2;OrgApacheHttpCookieClassLibrary"/>
		<rdfs:subClassOf rdf:resource="&java;JavaClassLibrary"/>
		<rdfs:comment xml:lang="en">JavaLibrary implementing the org.apache.http.cookie package for Android 2.3</rdfs:comment>
		<rdfs:comment xml:lang="OWLManchester">platform:implementsInterface some OrgApacheHttpCookieAPI</rdfs:comment>
	</owl:Class>
	<owl:Class rdf:about="&android-2_3;OrgApacheHttpCookieParamsClassLibrary">
		<owl:equivalentClass rdf:resource="&android-2_2;OrgApacheHttpCookieParamsClassLibrary"/>
		<rdfs:subClassOf rdf:resource="&java;JavaClassLibrary"/>
		<rdfs:comment xml:lang="en">JavaLibrary implementing the org.apache.http.cookie.params package for Android 2.3</rdfs:comment>
		<rdfs:comment xml:lang="OWLManchester">platform:implementsInterface some OrgApacheHttpCookieParamsAPI</rdfs:comment>
	</owl:Class>
	<owl:Class rdf:about="&android-2_3;OrgApacheHttpAuthClassLibrary">
		<owl:equivalentClass rdf:resource="&android-2_2;OrgApacheHttpAuthClassLibrary"/>
		<rdfs:subClassOf rdf:resource="&java;JavaClassLibrary"/>
		<rdfs:comment xml:lang="en">JavaLibrary implementing the org.apache.http.auth package for Android 2.3</rdfs:comment>
		<rdfs:comment xml:lang="OWLManchester">platform:implementsInterface some OrgApacheHttpAuthAPI</rdfs:comment>
	</owl:Class>
	<owl:Class rdf:about="&android-2_3;OrgApacheHttpAuthParamsClassLibrary">
		<owl:equivalentClass rdf:resource="&android-2_2;OrgApacheHttpAuthParamsClassLibrary"/>
		<rdfs:subClassOf rdf:resource="&java;JavaClassLibrary"/>
		<rdfs:comment xml:lang="en">JavaLibrary implementing the org.apache.http.auth.params package for Android 2.3</rdfs:comment>
		<rdfs:comment xml:lang="OWLManchester">platform:implementsInterface some OrgApacheHttpAuthParamsAPI</rdfs:comment>
	</owl:Class>
	<owl:Class rdf:about="&android-2_3;OrgApacheCommonsLoggingClassLibrary">
		<owl:equivalentClass rdf:resource="&android-2_2;OrgApacheCommonsLoggingClassLibrary"/>
		<rdfs:subClassOf rdf:resource="&java;JavaClassLibrary"/>
		<rdfs:comment xml:lang="en">JavaLibrary implementing the org.apache.commons.logging package for Android 2.3</rdfs:comment>
		<rdfs:comment xml:lang="OWLManchester">platform:implementsInterface some OrgApacheCommonsLoggingAPI</rdfs:comment>
	</owl:Class>
	<owl:Class rdf:about="&android-2_3;OrgJsonClassLibrary">
		<owl:equivalentClass rdf:resource="&android-2_2;OrgJsonClassLibrary"/>
		<rdfs:subClassOf rdf:resource="&java;JavaClassLibrary"/>
		<rdfs:comment xml:lang="en">JavaLibrary implementing the org.json package for Android 2.3</rdfs:comment>
		<rdfs:comment xml:lang="OWLManchester">platform:implementsInterface some OrgJsonAPI</rdfs:comment>
	</owl:Class>
	<owl:Class rdf:about="&android-2_3;DalvikBytecodeClassLibrary">
		<rdfs:subClassOf rdf:resource="&android-2_2;DalvikBytecodeClassLibrary"/>
		<rdfs:comment xml:lang="en">JavaLibrary implementing the dalvik.bytecode package for Android 2.3</rdfs:comment>
		<rdfs:comment xml:lang="OWLManchester">platform:implementsInterface some DalvikBytecodeAPI</rdfs:comment>
	</owl:Class>
	<owl:Class rdf:about="&android-2_3;DalvikAnnotationClassLibrary">
		<owl:equivalentClass rdf:resource="&android-2_2;DalvikAnnotationClassLibrary"/>
		<rdfs:subClassOf rdf:resource="&java;JavaClassLibrary"/>
		<rdfs:comment xml:lang="en">JavaLibrary implementing the dalvik.annotation package for Android 2.3</rdfs:comment>
		<rdfs:comment xml:lang="OWLManchester">platform:implementsInterface some DalvikAnnotationAPI</rdfs:comment>
	</owl:Class>
	<owl:Class rdf:about="&android-2_3;DalvikSystemClassLibrary">
		<rdfs:subClassOf rdf:resource="&java;JavaClassLibrary"/>
		<rdfs:comment xml:lang="en">JavaLibrary implementing the dalvik.system package for Android 2.3</rdfs:comment>
		<rdfs:comment xml:lang="OWLManchester">platform:implementsInterface some DalvikSystemAPI</rdfs:comment>
	</owl:Class>
	<owl:Class rdf:about="&android-2_3;JunitRunnerClassLibrary">
		<owl:equivalentClass rdf:resource="&android-2_2;JunitRunnerClassLibrary"/>
		<rdfs:subClassOf rdf:resource="&java;JavaClassLibrary"/>
		<rdfs:comment xml:lang="en">JavaLibrary implementing the junit.runner package for Android 2.3</rdfs:comment>
		<rdfs:comment xml:lang="OWLManchester">platform:implementsInterface some JunitRunnerAPI</rdfs:comment>
	</owl:Class>
	<owl:Class rdf:about="&android-2_3;JunitFrameworkClassLibrary">
		<owl:equivalentClass rdf:resource="&android-2_2;JunitFrameworkClassLibrary"/>
		<rdfs:subClassOf rdf:resource="&java;JavaClassLibrary"/>
		<rdfs:comment xml:lang="en">JavaLibrary implementing the junit.framework package for Android 2.3</rdfs:comment>
		<rdfs:comment xml:lang="OWLManchester">platform:implementsInterface some JunitFrameworkAPI</rdfs:comment>
	</owl:Class>
	<owl:Class rdf:about="&android-2_3;AndroidClassLibrary">
		<rdfs:subClassOf rdf:resource="&java;JavaClassLibrary"/>
		<rdfs:comment xml:lang="en">JavaLibrary implementing the android package for Android 2.3</rdfs:comment>
		<rdfs:comment xml:lang="OWLManchester">platform:implementsInterface some AndroidAPI</rdfs:comment>
	</owl:Class>
	<owl:Class rdf:about="&android-2_3;AndroidContentClassLibrary">
		<rdfs:subClassOf rdf:resource="&android-2_2;AndroidContentClassLibrary"/>
		<rdfs:comment xml:lang="en">JavaLibrary implementing the android.content package for Android 2.3</rdfs:comment>
		<rdfs:comment xml:lang="OWLManchester">platform:implementsInterface some AndroidContentAPI</rdfs:comment>
	</owl:Class>
	<owl:Class rdf:about="&android-2_3;AndroidContentPmClassLibrary">
		<rdfs:subClassOf rdf:resource="&android-2_2;AndroidContentPmClassLibrary"/>
		<rdfs:comment xml:lang="en">JavaLibrary implementing the android.content.pm package for Android 2.3</rdfs:comment>
		<rdfs:comment xml:lang="OWLManchester">platform:implementsInterface some AndroidContentPmAPI</rdfs:comment>
	</owl:Class>
	<owl:Class rdf:about="&android-2_3;AndroidContentResClassLibrary">
		<rdfs:subClassOf rdf:resource="&android-2_2;AndroidContentResClassLibrary"/>
		<rdfs:comment xml:lang="en">JavaLibrary implementing the android.content.res package for Android 2.3</rdfs:comment>
		<rdfs:comment xml:lang="OWLManchester">platform:implementsInterface some AndroidContentResAPI</rdfs:comment>
	</owl:Class>
	<owl:Class rdf:about="&android-2_3;AndroidOsClassLibrary">
		<rdfs:subClassOf rdf:resource="&android-2_2;AndroidOsClassLibrary"/>
		<rdfs:comment xml:lang="en">JavaLibrary implementing the android.os package for Android 2.3</rdfs:comment>
		<rdfs:comment xml:lang="OWLManchester">platform:implementsInterface some AndroidOsAPI</rdfs:comment>
	</owl:Class>
	<owl:Class rdf:about="&android-2_3;AndroidOsStorageClassLibrary">
		<rdfs:subClassOf rdf:resource="&java;JavaClassLibrary"/>
		<rdfs:comment xml:lang="en">JavaLibrary implementing the android.os.storage package for Android 2.3</rdfs:comment>
		<rdfs:comment xml:lang="OWLManchester">platform:implementsInterface some AndroidOsStorageAPI</rdfs:comment>
	</owl:Class>
	<owl:Class rdf:about="&android-2_3;AndroidAccountsClassLibrary">
		<rdfs:subClassOf rdf:resource="&android-2_2;AndroidAccountsClassLibrary"/>
		<rdfs:comment xml:lang="en">JavaLibrary implementing the android.accounts package for Android 2.3</rdfs:comment>
		<rdfs:comment xml:lang="OWLManchester">platform:implementsInterface some AndroidAccountsAPI</rdfs:comment>
	</owl:Class>
	<owl:Class rdf:about="&android-2_3;AndroidNetClassLibrary">
		<rdfs:subClassOf rdf:resource="&android-2_2;AndroidNetClassLibrary"/>
		<rdfs:comment xml:lang="en">JavaLibrary implementing the android.net package for Android 2.3</rdfs:comment>
		<rdfs:comment xml:lang="OWLManchester">platform:implementsInterface some AndroidNetAPI</rdfs:comment>
	</owl:Class>
	<owl:Class rdf:about="&android-2_3;AndroidNetHttpClassLibrary">
		<owl:equivalentClass rdf:resource="&android-2_2;AndroidNetHttpClassLibrary"/>
		<rdfs:subClassOf rdf:resource="&java;JavaClassLibrary"/>
		<rdfs:comment xml:lang="en">JavaLibrary implementing the android.net.http package for Android 2.3</rdfs:comment>
		<rdfs:comment xml:lang="OWLManchester">platform:implementsInterface some AndroidNetHttpAPI</rdfs:comment>
	</owl:Class>
	<owl:Class rdf:about="&android-2_3;AndroidNetSipClassLibrary">
		<rdfs:subClassOf rdf:resource="&java;JavaClassLibrary"/>
		<rdfs:comment xml:lang="en">JavaLibrary implementing the android.net.sip package for Android 2.3</rdfs:comment>
		<rdfs:comment xml:lang="OWLManchester">platform:implementsInterface some AndroidNetSipAPI</rdfs:comment>
	</owl:Class>
	<owl:Class rdf:about="&android-2_3;AndroidNetWifiClassLibrary">
		<rdfs:subClassOf rdf:resource="&android-2_2;AndroidNetWifiClassLibrary"/>
		<rdfs:comment xml:lang="en">JavaLibrary implementing the android.net.wifi package for Android 2.3</rdfs:comment>
		<rdfs:comment xml:lang="OWLManchester">platform:implementsInterface some AndroidNetWifiAPI</rdfs:comment>
	</owl:Class>
	<owl:Class rdf:about="&android-2_3;AndroidDatabaseClassLibrary">
		<rdfs:subClassOf rdf:resource="&android-2_2;AndroidDatabaseClassLibrary"/>
		<rdfs:comment xml:lang="en">JavaLibrary implementing the android.database package for Android 2.3</rdfs:comment>
		<rdfs:comment xml:lang="OWLManchester">platform:implementsInterface some AndroidDatabaseAPI</rdfs:comment>
	</owl:Class>
	<owl:Class rdf:about="&android-2_3;AndroidDatabaseSqliteClassLibrary">
		<owl:equivalentClass rdf:resource="&android-2_2;AndroidDatabaseSqliteClassLibrary"/>
		<rdfs:subClassOf rdf:resource="&java;JavaClassLibrary"/>
		<rdfs:comment xml:lang="en">JavaLibrary implementing the android.database.sqlite package for Android 2.3</rdfs:comment>
		<rdfs:comment xml:lang="OWLManchester">platform:implementsInterface some AndroidDatabaseSqliteAPI</rdfs:comment>
	</owl:Class>
	<owl:Class rdf:about="&android-2_3;AndroidUtilClassLibrary">
		<rdfs:subClassOf rdf:resource="&android-2_2;AndroidUtilClassLibrary"/>
		<rdfs:comment xml:lang="en">JavaLibrary implementing the android.util package for Android 2.3</rdfs:comment>
		<rdfs:comment xml:lang="OWLManchester">platform:implementsInterface some AndroidUtilAPI</rdfs:comment>
	</owl:Class>
	<owl:Class rdf:about="&android-2_3;AndroidGraphicsClassLibrary">
		<rdfs:subClassOf rdf:resource="&android-2_2;AndroidGraphicsClassLibrary"/>
		<rdfs:comment xml:lang="en">JavaLibrary implementing the android.graphics package for Android 2.3</rdfs:comment>
		<rdfs:comment xml:lang="OWLManchester">platform:implementsInterface some AndroidGraphicsAPI</rdfs:comment>
	</owl:Class>
	<owl:Class rdf:about="&android-2_3;AndroidGraphicsDrawableClassLibrary">
		<rdfs:subClassOf rdf:resource="&android-2_2;AndroidGraphicsDrawableClassLibrary"/>
		<rdfs:comment xml:lang="en">JavaLibrary implementing the android.graphics.drawable package for Android 2.3</rdfs:comment>
		<rdfs:comment xml:lang="OWLManchester">platform:implementsInterface some AndroidGraphicsDrawableAPI</rdfs:comment>
	</owl:Class>
	<owl:Class rdf:about="&android-2_3;AndroidGraphicsDrawableShapesClassLibrary">
		<owl:equivalentClass rdf:resource="&android-2_2;AndroidGraphicsDrawableShapesClassLibrary"/>
		<rdfs:subClassOf rdf:resource="&java;JavaClassLibrary"/>
		<rdfs:comment xml:lang="en">JavaLibrary implementing the android.graphics.drawable.shapes package for Android 2.3</rdfs:comment>
		<rdfs:comment xml:lang="OWLManchester">platform:implementsInterface some AndroidGraphicsDrawableShapesAPI</rdfs:comment>
	</owl:Class>
	<owl:Class rdf:about="&android-2_3;AndroidViewClassLibrary">
		<rdfs:subClassOf rdf:resource="&java;JavaClassLibrary"/>
		<rdfs:comment xml:lang="en">JavaLibrary implementing the android.view package for Android 2.3</rdfs:comment>
		<rdfs:comment xml:lang="OWLManchester">platform:implementsInterface some AndroidViewAPI</rdfs:comment>
	</owl:Class>
	<owl:Class rdf:about="&android-2_3;AndroidViewAccessibilityClassLibrary">
		<owl:equivalentClass rdf:resource="&android-2_2;AndroidViewAccessibilityClassLibrary"/>
		<rdfs:subClassOf rdf:resource="&java;JavaClassLibrary"/>
		<rdfs:comment xml:lang="en">JavaLibrary implementing the android.view.accessibility package for Android 2.3</rdfs:comment>
		<rdfs:comment xml:lang="OWLManchester">platform:implementsInterface some AndroidViewAccessibilityAPI</rdfs:comment>
	</owl:Class>
	<owl:Class rdf:about="&android-2_3;AndroidViewInputmethodClassLibrary">
		<rdfs:subClassOf rdf:resource="&android-2_2;AndroidViewInputmethodClassLibrary"/>
		<rdfs:comment xml:lang="en">JavaLibrary implementing the android.view.inputmethod package for Android 2.3</rdfs:comment>
		<rdfs:comment xml:lang="OWLManchester">platform:implementsInterface some AndroidViewInputmethodAPI</rdfs:comment>
	</owl:Class>
	<owl:Class rdf:about="&android-2_3;AndroidViewAnimationClassLibrary">
		<owl:equivalentClass rdf:resource="&android-2_2;AndroidViewAnimationClassLibrary"/>
		<rdfs:subClassOf rdf:resource="&java;JavaClassLibrary"/>
		<rdfs:comment xml:lang="en">JavaLibrary implementing the android.view.animation package for Android 2.3</rdfs:comment>
		<rdfs:comment xml:lang="OWLManchester">platform:implementsInterface some AndroidViewAnimationAPI</rdfs:comment>
	</owl:Class>
	<owl:Class rdf:about="&android-2_3;AndroidAccessibilityserviceClassLibrary">
		<rdfs:subClassOf rdf:resource="&android-2_2;AndroidAccessibilityserviceClassLibrary"/>
		<rdfs:comment xml:lang="en">JavaLibrary implementing the android.accessibilityservice package for Android 2.3</rdfs:comment>
		<rdfs:comment xml:lang="OWLManchester">platform:implementsInterface some AndroidAccessibilityserviceAPI</rdfs:comment>
	</owl:Class>
	<owl:Class rdf:about="&android-2_3;AndroidAppClassLibrary">
		<rdfs:subClassOf rdf:resource="&android-2_2;AndroidAppClassLibrary"/>
		<rdfs:comment xml:lang="en">JavaLibrary implementing the android.app package for Android 2.3</rdfs:comment>
		<rdfs:comment xml:lang="OWLManchester">platform:implementsInterface some AndroidAppAPI</rdfs:comment>
	</owl:Class>
	<owl:Class rdf:about="&android-2_3;AndroidAppBackupClassLibrary">
		<rdfs:subClassOf rdf:resource="&android-2_2;AndroidAppBackupClassLibrary"/>
		<rdfs:comment xml:lang="en">JavaLibrary implementing the android.app.backup package for Android 2.3</rdfs:comment>
		<rdfs:comment xml:lang="OWLManchester">platform:implementsInterface some AndroidAppBackupAPI</rdfs:comment>
	</owl:Class>
	<owl:Class rdf:about="&android-2_3;AndroidAppAdminClassLibrary">
		<rdfs:subClassOf rdf:resource="&android-2_2;AndroidAppAdminClassLibrary"/>
		<rdfs:comment xml:lang="en">JavaLibrary implementing the android.app.admin package for Android 2.3</rdfs:comment>
		<rdfs:comment xml:lang="OWLManchester">platform:implementsInterface some AndroidAppAdminAPI</rdfs:comment>
	</owl:Class>
	<owl:Class rdf:about="&android-2_3;AndroidTelephonyClassLibrary">
		<rdfs:subClassOf rdf:resource="&android-2_2;AndroidTelephonyClassLibrary"/>
		<rdfs:comment xml:lang="en">JavaLibrary implementing the android.telephony package for Android 2.3</rdfs:comment>
		<rdfs:comment xml:lang="OWLManchester">platform:implementsInterface some AndroidTelephonyAPI</rdfs:comment>
	</owl:Class>
	<owl:Class rdf:about="&android-2_3;AndroidTelephonyCdmaClassLibrary">
		<owl:equivalentClass rdf:resource="&android-2_2;AndroidTelephonyCdmaClassLibrary"/>
		<rdfs:subClassOf rdf:resource="&java;JavaClassLibrary"/>
		<rdfs:comment xml:lang="en">JavaLibrary implementing the android.telephony.cdma package for Android 2.3</rdfs:comment>
		<rdfs:comment xml:lang="OWLManchester">platform:implementsInterface some AndroidTelephonyCdmaAPI</rdfs:comment>
	</owl:Class>
	<owl:Class rdf:about="&android-2_3;AndroidTelephonyGsmClassLibrary">
		<rdfs:subClassOf rdf:resource="&android-2_2;AndroidTelephonyGsmClassLibrary"/>
		<rdfs:comment xml:lang="en">JavaLibrary implementing the android.telephony.gsm package for Android 2.3</rdfs:comment>
		<rdfs:comment xml:lang="OWLManchester">platform:implementsInterface some AndroidTelephonyGsmAPI</rdfs:comment>
	</owl:Class>
	<owl:Class rdf:about="&android-2_3;AndroidTextClassLibrary">
		<rdfs:subClassOf rdf:resource="&android-2_2;AndroidTextClassLibrary"/>
		<rdfs:comment xml:lang="en">JavaLibrary implementing the android.text package for Android 2.3</rdfs:comment>
		<rdfs:comment xml:lang="OWLManchester">platform:implementsInterface some AndroidTextAPI</rdfs:comment>
	</owl:Class>
	<owl:Class rdf:about="&android-2_3;AndroidTextUtilClassLibrary">
		<owl:equivalentClass rdf:resource="&android-2_2;AndroidTextUtilClassLibrary"/>
		<rdfs:subClassOf rdf:resource="&java;JavaClassLibrary"/>
		<rdfs:comment xml:lang="en">JavaLibrary implementing the android.text.util package for Android 2.3</rdfs:comment>
		<rdfs:comment xml:lang="OWLManchester">platform:implementsInterface some AndroidTextUtilAPI</rdfs:comment>
	</owl:Class>
	<owl:Class rdf:about="&android-2_3;AndroidTextFormatClassLibrary">
		<rdfs:subClassOf rdf:resource="&android-2_2;AndroidTextFormatClassLibrary"/>
		<rdfs:comment xml:lang="en">JavaLibrary implementing the android.text.format package for Android 2.3</rdfs:comment>
		<rdfs:comment xml:lang="OWLManchester">platform:implementsInterface some AndroidTextFormatAPI</rdfs:comment>
	</owl:Class>
	<owl:Class rdf:about="&android-2_3;AndroidTextMethodClassLibrary">
		<rdfs:subClassOf rdf:resource="&android-2_2;AndroidTextMethodClassLibrary"/>
		<rdfs:comment xml:lang="en">JavaLibrary implementing the android.text.method package for Android 2.3</rdfs:comment>
		<rdfs:comment xml:lang="OWLManchester">platform:implementsInterface some AndroidTextMethodAPI</rdfs:comment>
	</owl:Class>
	<owl:Class rdf:about="&android-2_3;AndroidTextStyleClassLibrary">
		<owl:equivalentClass rdf:resource="&android-2_2;AndroidTextStyleClassLibrary"/>
		<rdfs:subClassOf rdf:resource="&java;JavaClassLibrary"/>
		<rdfs:comment xml:lang="en">JavaLibrary implementing the android.text.style package for Android 2.3</rdfs:comment>
		<rdfs:comment xml:lang="OWLManchester">platform:implementsInterface some AndroidTextStyleAPI</rdfs:comment>
	</owl:Class>
	<owl:Class rdf:about="&android-2_3;AndroidGestureClassLibrary">
		<rdfs:subClassOf rdf:resource="&android-2_2;AndroidGestureClassLibrary"/>
		<rdfs:comment xml:lang="en">JavaLibrary implementing the android.gesture package for Android 2.3</rdfs:comment>
		<rdfs:comment xml:lang="OWLManchester">platform:implementsInterface some AndroidGestureAPI</rdfs:comment>
	</owl:Class>
	<owl:Class rdf:about="&android-2_3;AndroidWidgetClassLibrary">
		<rdfs:subClassOf rdf:resource="&android-2_2;AndroidWidgetClassLibrary"/>
		<rdfs:comment xml:lang="en">JavaLibrary implementing the android.widget package for Android 2.3</rdfs:comment>
		<rdfs:comment xml:lang="OWLManchester">platform:implementsInterface some AndroidWidgetAPI</rdfs:comment>
	</owl:Class>
	<owl:Class rdf:about="&android-2_3;AndroidLocationClassLibrary">
		<rdfs:subClassOf rdf:resource="&android-2_2;AndroidLocationClassLibrary"/>
		<rdfs:comment xml:lang="en">JavaLibrary implementing the android.location package for Android 2.3</rdfs:comment>
		<rdfs:comment xml:lang="OWLManchester">platform:implementsInterface some AndroidLocationAPI</rdfs:comment>
	</owl:Class>
	<owl:Class rdf:about="&android-2_3;AndroidHardwareClassLibrary">
		<rdfs:subClassOf rdf:resource="&android-2_2;AndroidHardwareClassLibrary"/>
		<rdfs:comment xml:lang="en">JavaLibrary implementing the android.hardware package for Android 2.3</rdfs:comment>
		<rdfs:comment xml:lang="OWLManchester">platform:implementsInterface some AndroidHardwareAPI</rdfs:comment>
	</owl:Class>
	<owl:Class rdf:about="&android-2_3;AndroidWebkitClassLibrary">
		<rdfs:subClassOf rdf:resource="&android-2_2;AndroidWebkitClassLibrary"/>
		<rdfs:comment xml:lang="en">JavaLibrary implementing the android.webkit package for Android 2.3</rdfs:comment>
		<rdfs:comment xml:lang="OWLManchester">platform:implementsInterface some AndroidWebkitAPI</rdfs:comment>
	</owl:Class>
	<owl:Class rdf:about="&android-2_3;AndroidTestClassLibrary">
		<rdfs:subClassOf rdf:resource="&android-2_2;AndroidTestClassLibrary"/>
		<rdfs:comment xml:lang="en">JavaLibrary implementing the android.test package for Android 2.3</rdfs:comment>
		<rdfs:comment xml:lang="OWLManchester">platform:implementsInterface some AndroidTestAPI</rdfs:comment>
	</owl:Class>
	<owl:Class rdf:about="&android-2_3;AndroidTestMockClassLibrary">
		<rdfs:subClassOf rdf:resource="&android-2_2;AndroidTestMockClassLibrary"/>
		<rdfs:comment xml:lang="en">JavaLibrary implementing the android.test.mock package for Android 2.3</rdfs:comment>
		<rdfs:comment xml:lang="OWLManchester">platform:implementsInterface some AndroidTestMockAPI</rdfs:comment>
	</owl:Class>
	<owl:Class rdf:about="&android-2_3;AndroidTestSuitebuilderClassLibrary">
		<owl:equivalentClass rdf:resource="&android-2_2;AndroidTestSuitebuilderClassLibrary"/>
		<rdfs:subClassOf rdf:resource="&java;JavaClassLibrary"/>
		<rdfs:comment xml:lang="en">JavaLibrary implementing the android.test.suitebuilder package for Android 2.3</rdfs:comment>
		<rdfs:comment xml:lang="OWLManchester">platform:implementsInterface some AndroidTestSuitebuilderAPI</rdfs:comment>
	</owl:Class>
	<owl:Class rdf:about="&android-2_3;AndroidTestSuitebuilderAnnotationClassLibrary">
		<owl:equivalentClass rdf:resource="&android-2_2;AndroidTestSuitebuilderAnnotationClassLibrary"/>
		<rdfs:subClassOf rdf:resource="&java;JavaClassLibrary"/>
		<rdfs:comment xml:lang="en">JavaLibrary implementing the android.test.suitebuilder.annotation package for Android 2.3</rdfs:comment>
		<rdfs:comment xml:lang="OWLManchester">platform:implementsInterface some AndroidTestSuitebuilderAnnotationAPI</rdfs:comment>
	</owl:Class>
	<owl:Class rdf:about="&android-2_3;AndroidPreferenceClassLibrary">
		<rdfs:subClassOf rdf:resource="&android-2_2;AndroidPreferenceClassLibrary"/>
		<rdfs:comment xml:lang="en">JavaLibrary implementing the android.preference package for Android 2.3</rdfs:comment>
		<rdfs:comment xml:lang="OWLManchester">platform:implementsInterface some AndroidPreferenceAPI</rdfs:comment>
	</owl:Class>
	<owl:Class rdf:about="&android-2_3;AndroidMediaClassLibrary">
		<rdfs:subClassOf rdf:resource="&android-2_2;AndroidMediaClassLibrary"/>
		<rdfs:comment xml:lang="en">JavaLibrary implementing the android.media package for Android 2.3</rdfs:comment>
		<rdfs:comment xml:lang="OWLManchester">platform:implementsInterface some AndroidMediaAPI</rdfs:comment>
	</owl:Class>
	<owl:Class rdf:about="&android-2_3;AndroidMediaAudiofxClassLibrary">
		<rdfs:subClassOf rdf:resource="&java;JavaClassLibrary"/>
		<rdfs:comment xml:lang="en">JavaLibrary implementing the android.media.audiofx package for Android 2.3</rdfs:comment>
		<rdfs:comment xml:lang="OWLManchester">platform:implementsInterface some AndroidMediaAudiofxAPI</rdfs:comment>
	</owl:Class>
	<owl:Class rdf:about="&android-2_3;AndroidInputmethodserviceClassLibrary">
		<rdfs:subClassOf rdf:resource="&android-2_2;AndroidInputmethodserviceClassLibrary"/>
		<rdfs:comment xml:lang="en">JavaLibrary implementing the android.inputmethodservice package for Android 2.3</rdfs:comment>
		<rdfs:comment xml:lang="OWLManchester">platform:implementsInterface some AndroidInputmethodserviceAPI</rdfs:comment>
	</owl:Class>
	<owl:Class rdf:about="&android-2_3;AndroidServiceWallpaperClassLibrary">
		<rdfs:subClassOf rdf:resource="&android-2_2;AndroidServiceWallpaperClassLibrary"/>
		<rdfs:comment xml:lang="en">JavaLibrary implementing the android.service.wallpaper package for Android 2.3</rdfs:comment>
		<rdfs:comment xml:lang="OWLManchester">platform:implementsInterface some AndroidServiceWallpaperAPI</rdfs:comment>
	</owl:Class>
	<owl:Class rdf:about="&android-2_3;AndroidBluetoothClassLibrary">
		<owl:equivalentClass rdf:resource="&android-2_2;AndroidBluetoothClassLibrary"/>
		<rdfs:subClassOf rdf:resource="&java;JavaClassLibrary"/>
		<rdfs:comment xml:lang="en">JavaLibrary implementing the android.bluetooth package for Android 2.3</rdfs:comment>
		<rdfs:comment xml:lang="OWLManchester">platform:implementsInterface some AndroidBluetoothAPI</rdfs:comment>
	</owl:Class>
	<owl:Class rdf:about="&android-2_3;AndroidNfcClassLibrary">
		<rdfs:subClassOf rdf:resource="&java;JavaClassLibrary"/>
		<rdfs:comment xml:lang="en">JavaLibrary implementing the android.nfc package for Android 2.3</rdfs:comment>
		<rdfs:comment xml:lang="OWLManchester">platform:implementsInterface some AndroidNfcAPI</rdfs:comment>
	</owl:Class>
	<owl:Class rdf:about="&android-2_3;AndroidProviderClassLibrary">
		<rdfs:subClassOf rdf:resource="&android-2_2;AndroidProviderClassLibrary"/>
		<rdfs:comment xml:lang="en">JavaLibrary implementing the android.provider package for Android 2.3</rdfs:comment>
		<rdfs:comment xml:lang="OWLManchester">platform:implementsInterface some AndroidProviderAPI</rdfs:comment>
	</owl:Class>
	<owl:Class rdf:about="&android-2_3;AndroidSaxClassLibrary">
		<owl:equivalentClass rdf:resource="&android-2_2;AndroidSaxClassLibrary"/>
		<rdfs:subClassOf rdf:resource="&java;JavaClassLibrary"/>
		<rdfs:comment xml:lang="en">JavaLibrary implementing the android.sax package for Android 2.3</rdfs:comment>
		<rdfs:comment xml:lang="OWLManchester">platform:implementsInterface some AndroidSaxAPI</rdfs:comment>
	</owl:Class>
	<owl:Class rdf:about="&android-2_3;AndroidAppwidgetClassLibrary">
		<rdfs:subClassOf rdf:resource="&android-2_2;AndroidAppwidgetClassLibrary"/>
		<rdfs:comment xml:lang="en">JavaLibrary implementing the android.appwidget package for Android 2.3</rdfs:comment>
		<rdfs:comment xml:lang="OWLManchester">platform:implementsInterface some AndroidAppwidgetAPI</rdfs:comment>
	</owl:Class>
	<owl:Class rdf:about="&android-2_3;AndroidOpenglClassLibrary">
		<rdfs:subClassOf rdf:resource="&android-2_2;AndroidOpenglClassLibrary"/>
		<rdfs:comment xml:lang="en">JavaLibrary implementing the android.opengl package for Android 2.3</rdfs:comment>
		<rdfs:comment xml:lang="OWLManchester">platform:implementsInterface some AndroidOpenglAPI</rdfs:comment>
	</owl:Class>
	<owl:Class rdf:about="&android-2_3;AndroidSpeechClassLibrary">
		<rdfs:subClassOf rdf:resource="&android-2_2;AndroidSpeechClassLibrary"/>
		<rdfs:comment xml:lang="en">JavaLibrary implementing the android.speech package for Android 2.3</rdfs:comment>
		<rdfs:comment xml:lang="OWLManchester">platform:implementsInterface some AndroidSpeechAPI</rdfs:comment>
	</owl:Class>
	<owl:Class rdf:about="&android-2_3;AndroidSpeechTtsClassLibrary">
		<owl:equivalentClass rdf:resource="&android-2_2;AndroidSpeechTtsClassLibrary"/>
		<rdfs:subClassOf rdf:resource="&java;JavaClassLibrary"/>
		<rdfs:comment xml:lang="en">JavaLibrary implementing the android.speech.tts package for Android 2.3</rdfs:comment>
		<rdfs:comment xml:lang="OWLManchester">platform:implementsInterface some AndroidSpeechTtsAPI</rdfs:comment>
	</owl:Class>
</rdf:RDF>
