<?xml version="1.0" encoding="ISO-8859-1"?>
<!DOCTYPE rdf:RDF [
	<!ENTITY platform "http://localhost/~dennis/platformkit/2010_1/platform.owl#">
	<!ENTITY ns_33 "http://localhost/~dennis/platformkit/2010_1/">
	<!ENTITY xsd "http://www.w3.org/2001/XMLSchema#">
	<!ENTITY isa "http://localhost/~dennis/platformkit/2010_1/isa.owl#">
	<!ENTITY java-se-6 "http://soft.vub.ac.be/platformkit/2010/1/java-se-6.owl#">
	<!ENTITY android-2_1 "http://soft.vub.ac.be/platformkit/2010/1/android-2_1.owl#">
	<!ENTITY java "http://localhost/~dennis/platformkit/2010_1/java.owl#">
	<!ENTITY android-1_6 "http://soft.vub.ac.be/platformkit/2010/1/android-1_6.owl#">
	<!ENTITY rdfs "http://www.w3.org/2000/01/rdf-schema#">
	<!ENTITY rdf "http://www.w3.org/1999/02/22-rdf-syntax-ns#">
	<!ENTITY owl "http://www.w3.org/2002/07/owl#">
]>
<rdf:RDF
	 xmlns:platform="&platform;"
	 xmlns:ns_33="&ns_33;"
	 xmlns:xsd="&xsd;"
	 xmlns:isa="&isa;"
	 xmlns:java-se-6="&java-se-6;"
	 xmlns:android-2_1="&android-2_1;"
	 xmlns:java="&java;"
	 xmlns:android-1_6="&android-1_6;"
	 xmlns:rdfs="&rdfs;"
	 xmlns:rdf="&rdf;"
	 xmlns:owl="&owl;"
>

	<owl:Ontology rdf:about="http://soft.vub.ac.be/platformkit/2010/1/android-2_1.owl#">
		<owl:versionInfo>$Id: UML2ToPackageAPIOntology.atl 8082 2010-03-18 21:11:00Z dwagelaa $</owl:versionInfo>
		<owl:imports rdf:resource="http://localhost/~dennis/platformkit/2010_1/platform.owl"/>
		<owl:imports rdf:resource="http://localhost/~dennis/platformkit/2010_1/java.owl"/>
		<owl:imports rdf:resource="http://soft.vub.ac.be/platformkit/2010/1/android-1_6.owl#"/>
		<owl:imports rdf:resource="http://localhost/~dennis/platformkit/2010_1/isa.owl"/>
		<owl:imports rdf:resource="http://soft.vub.ac.be/platformkit/2010/1/java-se-6.owl#"/>
		<rdfs:comment xml:lang="en">Generated by [UML2ToSimplifiedPackageAPIOntology.atl 8080 2010-03-18 10:46:40Z dwagelaa], [UML2ToPackageAPIOntology.atl 8082 2010-03-18 21:11:00Z dwagelaa], [UML2ToAPIOntology.atl 8086 2010-03-19 09:49:17Z dwagelaa], and [UML2Comparison.atl 8326 2010-11-11 13:32:14Z dwagelaa]</rdfs:comment>
		<rdfs:comment>Dennis Wagelaar &lt;dennis.wagelaar@vub.ac.be&gt;</rdfs:comment>
		<rdfs:comment xml:lang="en">&#169; 2010, Vrije Universiteit Brussel. All rights reserved.</rdfs:comment>
		<rdfs:label xml:lang="en">Android 2.1</rdfs:label>
	</owl:Ontology>
	<owl:Class rdf:about="&android-2_1;Android2_1API">
		<rdfs:subClassOf rdf:resource="&android-2_1;AndroidAPI"/>
		<rdfs:subClassOf rdf:resource="&android-2_1;AndroidAccessibilityserviceAPI"/>
		<rdfs:subClassOf rdf:resource="&android-2_1;AndroidAppAPI"/>
		<rdfs:subClassOf rdf:resource="&android-2_1;AndroidViewAPI"/>
		<rdfs:subClassOf rdf:resource="&android-2_1;AndroidViewAccessibilityAPI"/>
		<rdfs:subClassOf rdf:resource="&android-2_1;AndroidViewInputmethodAPI"/>
		<rdfs:subClassOf rdf:resource="&android-2_1;AndroidViewAnimationAPI"/>
		<rdfs:subClassOf rdf:resource="&android-2_1;AndroidContentAPI"/>
		<rdfs:subClassOf rdf:resource="&android-2_1;AndroidContentResAPI"/>
		<rdfs:subClassOf rdf:resource="&android-2_1;AndroidContentPmAPI"/>
		<rdfs:subClassOf rdf:resource="&android-2_1;AndroidOsAPI"/>
		<rdfs:subClassOf rdf:resource="&android-2_1;AndroidAccountsAPI"/>
		<rdfs:subClassOf rdf:resource="&android-2_1;AndroidGraphicsAPI"/>
		<rdfs:subClassOf rdf:resource="&android-2_1;AndroidGraphicsDrawableAPI"/>
		<rdfs:subClassOf rdf:resource="&android-2_1;AndroidGraphicsDrawableShapesAPI"/>
		<rdfs:subClassOf rdf:resource="&android-2_1;AndroidNetAPI"/>
		<rdfs:subClassOf rdf:resource="&android-2_1;AndroidNetHttpAPI"/>
		<rdfs:subClassOf rdf:resource="&android-2_1;AndroidNetWifiAPI"/>
		<rdfs:subClassOf rdf:resource="&android-2_1;AndroidDatabaseAPI"/>
		<rdfs:subClassOf rdf:resource="&android-2_1;AndroidDatabaseSqliteAPI"/>
		<rdfs:subClassOf rdf:resource="&android-2_1;AndroidUtilAPI"/>
		<rdfs:subClassOf rdf:resource="&android-2_1;AndroidWidgetAPI"/>
		<rdfs:subClassOf rdf:resource="&android-2_1;AndroidAppwidgetAPI"/>
		<rdfs:subClassOf rdf:resource="&android-2_1;AndroidBluetoothAPI"/>
		<rdfs:subClassOf rdf:resource="&android-2_1;AndroidGestureAPI"/>
		<rdfs:subClassOf rdf:resource="&android-2_1;AndroidHardwareAPI"/>
		<rdfs:subClassOf rdf:resource="&android-2_1;AndroidInputmethodserviceAPI"/>
		<rdfs:subClassOf rdf:resource="&android-2_1;AndroidLocationAPI"/>
		<rdfs:subClassOf rdf:resource="&android-2_1;AndroidMediaAPI"/>
		<rdfs:subClassOf rdf:resource="&android-2_1;AndroidOpenglAPI"/>
		<rdfs:subClassOf rdf:resource="&android-2_1;AndroidPreferenceAPI"/>
		<rdfs:subClassOf rdf:resource="&android-2_1;AndroidProviderAPI"/>
		<rdfs:subClassOf rdf:resource="&android-2_1;AndroidWebkitAPI"/>
		<rdfs:subClassOf rdf:resource="&android-2_1;AndroidSaxAPI"/>
		<rdfs:subClassOf rdf:resource="&android-2_1;AndroidServiceWallpaperAPI"/>
		<rdfs:subClassOf rdf:resource="&android-2_1;AndroidSpeechAPI"/>
		<rdfs:subClassOf rdf:resource="&android-2_1;AndroidSpeechTtsAPI"/>
		<rdfs:subClassOf rdf:resource="&android-2_1;AndroidTelephonyAPI"/>
		<rdfs:subClassOf rdf:resource="&android-2_1;AndroidTelephonyCdmaAPI"/>
		<rdfs:subClassOf rdf:resource="&android-2_1;AndroidTelephonyGsmAPI"/>
		<rdfs:subClassOf rdf:resource="&android-2_1;AndroidTextAPI"/>
		<rdfs:subClassOf rdf:resource="&android-2_1;AndroidTextFormatAPI"/>
		<rdfs:subClassOf rdf:resource="&android-2_1;AndroidTextMethodAPI"/>
		<rdfs:subClassOf rdf:resource="&android-2_1;AndroidTextStyleAPI"/>
		<rdfs:subClassOf rdf:resource="&android-2_1;AndroidTextUtilAPI"/>
		<rdfs:subClassOf rdf:resource="&android-2_1;AndroidTestAPI"/>
		<rdfs:subClassOf rdf:resource="&android-2_1;AndroidTestMockAPI"/>
		<rdfs:subClassOf rdf:resource="&android-2_1;AndroidTestSuitebuilderAPI"/>
		<rdfs:subClassOf rdf:resource="&android-2_1;AndroidTestSuitebuilderAnnotationAPI"/>
		<rdfs:subClassOf rdf:resource="&android-2_1;JavaLangAPI"/>
		<rdfs:subClassOf rdf:resource="&android-2_1;JavaLangAnnotationAPI"/>
		<rdfs:subClassOf rdf:resource="&android-2_1;JavaLangReflectAPI"/>
		<rdfs:subClassOf rdf:resource="&android-2_1;JavaLangRefAPI"/>
		<rdfs:subClassOf rdf:resource="&android-2_1;JavaUtilAPI"/>
		<rdfs:subClassOf rdf:resource="&android-2_1;JavaUtilConcurrentAPI"/>
		<rdfs:subClassOf rdf:resource="&android-2_1;JavaUtilConcurrentAtomicAPI"/>
		<rdfs:subClassOf rdf:resource="&android-2_1;JavaUtilConcurrentLocksAPI"/>
		<rdfs:subClassOf rdf:resource="&android-2_1;JavaUtilRegexAPI"/>
		<rdfs:subClassOf rdf:resource="&android-2_1;JavaUtilJarAPI"/>
		<rdfs:subClassOf rdf:resource="&android-2_1;JavaUtilZipAPI"/>
		<rdfs:subClassOf rdf:resource="&android-2_1;JavaUtilLoggingAPI"/>
		<rdfs:subClassOf rdf:resource="&android-2_1;JavaUtilPrefsAPI"/>
		<rdfs:subClassOf rdf:resource="&android-2_1;JavaIoAPI"/>
		<rdfs:subClassOf rdf:resource="&android-2_1;JavaNioAPI"/>
		<rdfs:subClassOf rdf:resource="&android-2_1;JavaNioChannelsAPI"/>
		<rdfs:subClassOf rdf:resource="&android-2_1;JavaNioChannelsSpiAPI"/>
		<rdfs:subClassOf rdf:resource="&android-2_1;JavaNioCharsetAPI"/>
		<rdfs:subClassOf rdf:resource="&android-2_1;JavaNioCharsetSpiAPI"/>
		<rdfs:subClassOf rdf:resource="&android-2_1;JavaNetAPI"/>
		<rdfs:subClassOf rdf:resource="&android-2_1;JavaSecurityAPI"/>
		<rdfs:subClassOf rdf:resource="&android-2_1;JavaSecurityCertAPI"/>
		<rdfs:subClassOf rdf:resource="&android-2_1;JavaSecuritySpecAPI"/>
		<rdfs:subClassOf rdf:resource="&android-2_1;JavaSecurityAclAPI"/>
		<rdfs:subClassOf rdf:resource="&android-2_1;JavaSecurityInterfacesAPI"/>
		<rdfs:subClassOf rdf:resource="&android-2_1;JavaTextAPI"/>
		<rdfs:subClassOf rdf:resource="&android-2_1;JavaAwtFontAPI"/>
		<rdfs:subClassOf rdf:resource="&android-2_1;JavaBeansAPI"/>
		<rdfs:subClassOf rdf:resource="&android-2_1;JavaMathAPI"/>
		<rdfs:subClassOf rdf:resource="&android-2_1;JavaSqlAPI"/>
		<rdfs:subClassOf rdf:resource="&android-2_1;OrgXmlpullV1API"/>
		<rdfs:subClassOf rdf:resource="&android-2_1;OrgXmlpullV1Sax2API"/>
		<rdfs:subClassOf rdf:resource="&android-2_1;OrgXmlSaxAPI"/>
		<rdfs:subClassOf rdf:resource="&android-2_1;OrgXmlSaxHelpersAPI"/>
		<rdfs:subClassOf rdf:resource="&android-2_1;OrgXmlSaxExtAPI"/>
		<rdfs:subClassOf rdf:resource="&android-2_1;OrgW3cDomAPI"/>
		<rdfs:subClassOf rdf:resource="&android-2_1;OrgApacheCommonsLoggingAPI"/>
		<rdfs:subClassOf rdf:resource="&android-2_1;OrgApacheHttpAPI"/>
		<rdfs:subClassOf rdf:resource="&android-2_1;OrgApacheHttpProtocolAPI"/>
		<rdfs:subClassOf rdf:resource="&android-2_1;OrgApacheHttpUtilAPI"/>
		<rdfs:subClassOf rdf:resource="&android-2_1;OrgApacheHttpParamsAPI"/>
		<rdfs:subClassOf rdf:resource="&android-2_1;OrgApacheHttpAuthAPI"/>
		<rdfs:subClassOf rdf:resource="&android-2_1;OrgApacheHttpAuthParamsAPI"/>
		<rdfs:subClassOf rdf:resource="&android-2_1;OrgApacheHttpClientAPI"/>
		<rdfs:subClassOf rdf:resource="&android-2_1;OrgApacheHttpClientMethodsAPI"/>
		<rdfs:subClassOf rdf:resource="&android-2_1;OrgApacheHttpClientEntityAPI"/>
		<rdfs:subClassOf rdf:resource="&android-2_1;OrgApacheHttpClientParamsAPI"/>
		<rdfs:subClassOf rdf:resource="&android-2_1;OrgApacheHttpClientProtocolAPI"/>
		<rdfs:subClassOf rdf:resource="&android-2_1;OrgApacheHttpClientUtilsAPI"/>
		<rdfs:subClassOf rdf:resource="&android-2_1;OrgApacheHttpCookieAPI"/>
		<rdfs:subClassOf rdf:resource="&android-2_1;OrgApacheHttpCookieParamsAPI"/>
		<rdfs:subClassOf rdf:resource="&android-2_1;OrgApacheHttpConnAPI"/>
		<rdfs:subClassOf rdf:resource="&android-2_1;OrgApacheHttpConnParamsAPI"/>
		<rdfs:subClassOf rdf:resource="&android-2_1;OrgApacheHttpConnSchemeAPI"/>
		<rdfs:subClassOf rdf:resource="&android-2_1;OrgApacheHttpConnRoutingAPI"/>
		<rdfs:subClassOf rdf:resource="&android-2_1;OrgApacheHttpConnSslAPI"/>
		<rdfs:subClassOf rdf:resource="&android-2_1;OrgApacheHttpConnUtilAPI"/>
		<rdfs:subClassOf rdf:resource="&android-2_1;OrgApacheHttpEntityAPI"/>
		<rdfs:subClassOf rdf:resource="&android-2_1;OrgApacheHttpMessageAPI"/>
		<rdfs:subClassOf rdf:resource="&android-2_1;OrgApacheHttpImplAPI"/>
		<rdfs:subClassOf rdf:resource="&android-2_1;OrgApacheHttpImplEntityAPI"/>
		<rdfs:subClassOf rdf:resource="&android-2_1;OrgApacheHttpImplAuthAPI"/>
		<rdfs:subClassOf rdf:resource="&android-2_1;OrgApacheHttpImplClientAPI"/>
		<rdfs:subClassOf rdf:resource="&android-2_1;OrgApacheHttpImplConnAPI"/>
		<rdfs:subClassOf rdf:resource="&android-2_1;OrgApacheHttpImplConnTsccmAPI"/>
		<rdfs:subClassOf rdf:resource="&android-2_1;OrgApacheHttpImplIoAPI"/>
		<rdfs:subClassOf rdf:resource="&android-2_1;OrgApacheHttpImplCookieAPI"/>
		<rdfs:subClassOf rdf:resource="&android-2_1;OrgApacheHttpIoAPI"/>
		<rdfs:subClassOf rdf:resource="&android-2_1;OrgJsonAPI"/>
		<rdfs:subClassOf rdf:resource="&android-2_1;JavaxMicroeditionKhronosOpenglesAPI"/>
		<rdfs:subClassOf rdf:resource="&android-2_1;JavaxMicroeditionKhronosEglAPI"/>
		<rdfs:subClassOf rdf:resource="&android-2_1;JavaxNetAPI"/>
		<rdfs:subClassOf rdf:resource="&android-2_1;JavaxNetSslAPI"/>
		<rdfs:subClassOf rdf:resource="&android-2_1;JavaxSecurityAuthAPI"/>
		<rdfs:subClassOf rdf:resource="&android-2_1;JavaxSecurityAuthCallbackAPI"/>
		<rdfs:subClassOf rdf:resource="&android-2_1;JavaxSecurityAuthX500API"/>
		<rdfs:subClassOf rdf:resource="&android-2_1;JavaxSecurityAuthLoginAPI"/>
		<rdfs:subClassOf rdf:resource="&android-2_1;JavaxSecurityCertAPI"/>
		<rdfs:subClassOf rdf:resource="&android-2_1;JavaxCryptoAPI"/>
		<rdfs:subClassOf rdf:resource="&android-2_1;JavaxCryptoInterfacesAPI"/>
		<rdfs:subClassOf rdf:resource="&android-2_1;JavaxCryptoSpecAPI"/>
		<rdfs:subClassOf rdf:resource="&android-2_1;JavaxSqlAPI"/>
		<rdfs:subClassOf rdf:resource="&android-2_1;JavaxXmlAPI"/>
		<rdfs:subClassOf rdf:resource="&android-2_1;JavaxXmlParsersAPI"/>
		<rdfs:subClassOf rdf:resource="&android-2_1;JunitFrameworkAPI"/>
		<rdfs:subClassOf rdf:resource="&android-2_1;JunitRunnerAPI"/>
		<rdfs:subClassOf rdf:resource="&android-2_1;DalvikAnnotationAPI"/>
		<rdfs:subClassOf rdf:resource="&android-2_1;DalvikBytecodeAPI"/>
		<rdfs:subClassOf rdf:resource="&android-2_1;DalvikSystemAPI"/>
		<rdfs:comment xml:lang="en">Android 2.1 API</rdfs:comment>
		<rdfs:comment xml:lang="OWLManchester">platform:comprisesInterfacePart some Android and platform:comprisesInterfacePart some AndroidAccessibilityservice and platform:comprisesInterfacePart some AndroidApp and platform:comprisesInterfacePart some AndroidView and platform:comprisesInterfacePart some AndroidViewAccessibility and platform:comprisesInterfacePart some AndroidViewInputmethod and platform:comprisesInterfacePart some AndroidViewAnimation and platform:comprisesInterfacePart some AndroidContent and platform:comprisesInterfacePart some AndroidContentRes and platform:comprisesInterfacePart some AndroidContentPm and platform:comprisesInterfacePart some AndroidOs and platform:comprisesInterfacePart some AndroidAccounts and platform:comprisesInterfacePart some AndroidGraphics and platform:comprisesInterfacePart some AndroidGraphicsDrawable and platform:comprisesInterfacePart some AndroidGraphicsDrawableShapes and platform:comprisesInterfacePart some AndroidNet and platform:comprisesInterfacePart some AndroidNetHttp and platform:comprisesInterfacePart some AndroidNetWifi and platform:comprisesInterfacePart some AndroidDatabase and platform:comprisesInterfacePart some AndroidDatabaseSqlite and platform:comprisesInterfacePart some AndroidUtil and platform:comprisesInterfacePart some AndroidWidget and platform:comprisesInterfacePart some AndroidAppwidget and platform:comprisesInterfacePart some AndroidBluetooth and platform:comprisesInterfacePart some AndroidGesture and platform:comprisesInterfacePart some AndroidHardware and platform:comprisesInterfacePart some AndroidInputmethodservice and platform:comprisesInterfacePart some AndroidLocation and platform:comprisesInterfacePart some AndroidMedia and platform:comprisesInterfacePart some AndroidOpengl and platform:comprisesInterfacePart some AndroidPreference and platform:comprisesInterfacePart some AndroidProvider and platform:comprisesInterfacePart some AndroidWebkit and platform:comprisesInterfacePart some AndroidSax and platform:comprisesInterfacePart some AndroidServiceWallpaper and platform:comprisesInterfacePart some AndroidSpeech and platform:comprisesInterfacePart some AndroidSpeechTts and platform:comprisesInterfacePart some AndroidTelephony and platform:comprisesInterfacePart some AndroidTelephonyCdma and platform:comprisesInterfacePart some AndroidTelephonyGsm and platform:comprisesInterfacePart some AndroidText and platform:comprisesInterfacePart some AndroidTextFormat and platform:comprisesInterfacePart some AndroidTextMethod and platform:comprisesInterfacePart some AndroidTextStyle and platform:comprisesInterfacePart some AndroidTextUtil and platform:comprisesInterfacePart some AndroidTest and platform:comprisesInterfacePart some AndroidTestMock and platform:comprisesInterfacePart some AndroidTestSuitebuilder and platform:comprisesInterfacePart some AndroidTestSuitebuilderAnnotation and platform:comprisesInterfacePart some JavaLang and platform:comprisesInterfacePart some JavaLangAnnotation and platform:comprisesInterfacePart some JavaLangReflect and platform:comprisesInterfacePart some JavaLangRef and platform:comprisesInterfacePart some JavaUtil and platform:comprisesInterfacePart some JavaUtilConcurrent and platform:comprisesInterfacePart some JavaUtilConcurrentAtomic and platform:comprisesInterfacePart some JavaUtilConcurrentLocks and platform:comprisesInterfacePart some JavaUtilRegex and platform:comprisesInterfacePart some JavaUtilJar and platform:comprisesInterfacePart some JavaUtilZip and platform:comprisesInterfacePart some JavaUtilLogging and platform:comprisesInterfacePart some JavaUtilPrefs and platform:comprisesInterfacePart some JavaIo and platform:comprisesInterfacePart some JavaNio and platform:comprisesInterfacePart some JavaNioChannels and platform:comprisesInterfacePart some JavaNioChannelsSpi and platform:comprisesInterfacePart some JavaNioCharset and platform:comprisesInterfacePart some JavaNioCharsetSpi and platform:comprisesInterfacePart some JavaNet and platform:comprisesInterfacePart some JavaSecurity and platform:comprisesInterfacePart some JavaSecurityCert and platform:comprisesInterfacePart some JavaSecuritySpec and platform:comprisesInterfacePart some JavaSecurityAcl and platform:comprisesInterfacePart some JavaSecurityInterfaces and platform:comprisesInterfacePart some JavaText and platform:comprisesInterfacePart some JavaAwtFont and platform:comprisesInterfacePart some JavaBeans and platform:comprisesInterfacePart some JavaMath and platform:comprisesInterfacePart some JavaSql and platform:comprisesInterfacePart some OrgXmlpullV1 and platform:comprisesInterfacePart some OrgXmlpullV1Sax2 and platform:comprisesInterfacePart some OrgXmlSax and platform:comprisesInterfacePart some OrgXmlSaxHelpers and platform:comprisesInterfacePart some OrgXmlSaxExt and platform:comprisesInterfacePart some OrgW3cDom and platform:comprisesInterfacePart some OrgApacheCommonsLogging and platform:comprisesInterfacePart some OrgApacheHttp and platform:comprisesInterfacePart some OrgApacheHttpProtocol and platform:comprisesInterfacePart some OrgApacheHttpUtil and platform:comprisesInterfacePart some OrgApacheHttpParams and platform:comprisesInterfacePart some OrgApacheHttpAuth and platform:comprisesInterfacePart some OrgApacheHttpAuthParams and platform:comprisesInterfacePart some OrgApacheHttpClient and platform:comprisesInterfacePart some OrgApacheHttpClientMethods and platform:comprisesInterfacePart some OrgApacheHttpClientEntity and platform:comprisesInterfacePart some OrgApacheHttpClientParams and platform:comprisesInterfacePart some OrgApacheHttpClientProtocol and platform:comprisesInterfacePart some OrgApacheHttpClientUtils and platform:comprisesInterfacePart some OrgApacheHttpCookie and platform:comprisesInterfacePart some OrgApacheHttpCookieParams and platform:comprisesInterfacePart some OrgApacheHttpConn and platform:comprisesInterfacePart some OrgApacheHttpConnParams and platform:comprisesInterfacePart some OrgApacheHttpConnScheme and platform:comprisesInterfacePart some OrgApacheHttpConnRouting and platform:comprisesInterfacePart some OrgApacheHttpConnSsl and platform:comprisesInterfacePart some OrgApacheHttpConnUtil and platform:comprisesInterfacePart some OrgApacheHttpEntity and platform:comprisesInterfacePart some OrgApacheHttpMessage and platform:comprisesInterfacePart some OrgApacheHttpImpl and platform:comprisesInterfacePart some OrgApacheHttpImplEntity and platform:comprisesInterfacePart some OrgApacheHttpImplAuth and platform:comprisesInterfacePart some OrgApacheHttpImplClient and platform:comprisesInterfacePart some OrgApacheHttpImplConn and platform:comprisesInterfacePart some OrgApacheHttpImplConnTsccm and platform:comprisesInterfacePart some OrgApacheHttpImplIo and platform:comprisesInterfacePart some OrgApacheHttpImplCookie and platform:comprisesInterfacePart some OrgApacheHttpIo and platform:comprisesInterfacePart some OrgJson and platform:comprisesInterfacePart some JavaxMicroeditionKhronosOpengles and platform:comprisesInterfacePart some JavaxMicroeditionKhronosEgl and platform:comprisesInterfacePart some JavaxNet and platform:comprisesInterfacePart some JavaxNetSsl and platform:comprisesInterfacePart some JavaxSecurityAuth and platform:comprisesInterfacePart some JavaxSecurityAuthCallback and platform:comprisesInterfacePart some JavaxSecurityAuthX500 and platform:comprisesInterfacePart some JavaxSecurityAuthLogin and platform:comprisesInterfacePart some JavaxSecurityCert and platform:comprisesInterfacePart some JavaxCrypto and platform:comprisesInterfacePart some JavaxCryptoInterfaces and platform:comprisesInterfacePart some JavaxCryptoSpec and platform:comprisesInterfacePart some JavaxSql and platform:comprisesInterfacePart some JavaxXml and platform:comprisesInterfacePart some JavaxXmlParsers and platform:comprisesInterfacePart some JunitFramework and platform:comprisesInterfacePart some JunitRunner and platform:comprisesInterfacePart some DalvikAnnotation and platform:comprisesInterfacePart some DalvikBytecode and platform:comprisesInterfacePart some DalvikSystem</rdfs:comment>
	</owl:Class>
	<owl:Class rdf:about="&android-2_1;Android2_1ClassLibrary">
		<rdfs:subClassOf rdf:resource="&android-2_1;AndroidClassLibrary"/>
		<rdfs:subClassOf rdf:resource="&android-2_1;AndroidAccessibilityserviceClassLibrary"/>
		<rdfs:subClassOf rdf:resource="&android-2_1;AndroidAppClassLibrary"/>
		<rdfs:subClassOf rdf:resource="&android-2_1;AndroidViewClassLibrary"/>
		<rdfs:subClassOf rdf:resource="&android-2_1;AndroidViewAccessibilityClassLibrary"/>
		<rdfs:subClassOf rdf:resource="&android-2_1;AndroidViewInputmethodClassLibrary"/>
		<rdfs:subClassOf rdf:resource="&android-2_1;AndroidViewAnimationClassLibrary"/>
		<rdfs:subClassOf rdf:resource="&android-2_1;AndroidContentClassLibrary"/>
		<rdfs:subClassOf rdf:resource="&android-2_1;AndroidContentResClassLibrary"/>
		<rdfs:subClassOf rdf:resource="&android-2_1;AndroidContentPmClassLibrary"/>
		<rdfs:subClassOf rdf:resource="&android-2_1;AndroidOsClassLibrary"/>
		<rdfs:subClassOf rdf:resource="&android-2_1;AndroidAccountsClassLibrary"/>
		<rdfs:subClassOf rdf:resource="&android-2_1;AndroidGraphicsClassLibrary"/>
		<rdfs:subClassOf rdf:resource="&android-2_1;AndroidGraphicsDrawableClassLibrary"/>
		<rdfs:subClassOf rdf:resource="&android-2_1;AndroidGraphicsDrawableShapesClassLibrary"/>
		<rdfs:subClassOf rdf:resource="&android-2_1;AndroidNetClassLibrary"/>
		<rdfs:subClassOf rdf:resource="&android-2_1;AndroidNetHttpClassLibrary"/>
		<rdfs:subClassOf rdf:resource="&android-2_1;AndroidNetWifiClassLibrary"/>
		<rdfs:subClassOf rdf:resource="&android-2_1;AndroidDatabaseClassLibrary"/>
		<rdfs:subClassOf rdf:resource="&android-2_1;AndroidDatabaseSqliteClassLibrary"/>
		<rdfs:subClassOf rdf:resource="&android-2_1;AndroidUtilClassLibrary"/>
		<rdfs:subClassOf rdf:resource="&android-2_1;AndroidWidgetClassLibrary"/>
		<rdfs:subClassOf rdf:resource="&android-2_1;AndroidAppwidgetClassLibrary"/>
		<rdfs:subClassOf rdf:resource="&android-2_1;AndroidBluetoothClassLibrary"/>
		<rdfs:subClassOf rdf:resource="&android-2_1;AndroidGestureClassLibrary"/>
		<rdfs:subClassOf rdf:resource="&android-2_1;AndroidHardwareClassLibrary"/>
		<rdfs:subClassOf rdf:resource="&android-2_1;AndroidInputmethodserviceClassLibrary"/>
		<rdfs:subClassOf rdf:resource="&android-2_1;AndroidLocationClassLibrary"/>
		<rdfs:subClassOf rdf:resource="&android-2_1;AndroidMediaClassLibrary"/>
		<rdfs:subClassOf rdf:resource="&android-2_1;AndroidOpenglClassLibrary"/>
		<rdfs:subClassOf rdf:resource="&android-2_1;AndroidPreferenceClassLibrary"/>
		<rdfs:subClassOf rdf:resource="&android-2_1;AndroidProviderClassLibrary"/>
		<rdfs:subClassOf rdf:resource="&android-2_1;AndroidWebkitClassLibrary"/>
		<rdfs:subClassOf rdf:resource="&android-2_1;AndroidSaxClassLibrary"/>
		<rdfs:subClassOf rdf:resource="&android-2_1;AndroidServiceWallpaperClassLibrary"/>
		<rdfs:subClassOf rdf:resource="&android-2_1;AndroidSpeechClassLibrary"/>
		<rdfs:subClassOf rdf:resource="&android-2_1;AndroidSpeechTtsClassLibrary"/>
		<rdfs:subClassOf rdf:resource="&android-2_1;AndroidTelephonyClassLibrary"/>
		<rdfs:subClassOf rdf:resource="&android-2_1;AndroidTelephonyCdmaClassLibrary"/>
		<rdfs:subClassOf rdf:resource="&android-2_1;AndroidTelephonyGsmClassLibrary"/>
		<rdfs:subClassOf rdf:resource="&android-2_1;AndroidTextClassLibrary"/>
		<rdfs:subClassOf rdf:resource="&android-2_1;AndroidTextFormatClassLibrary"/>
		<rdfs:subClassOf rdf:resource="&android-2_1;AndroidTextMethodClassLibrary"/>
		<rdfs:subClassOf rdf:resource="&android-2_1;AndroidTextStyleClassLibrary"/>
		<rdfs:subClassOf rdf:resource="&android-2_1;AndroidTextUtilClassLibrary"/>
		<rdfs:subClassOf rdf:resource="&android-2_1;AndroidTestClassLibrary"/>
		<rdfs:subClassOf rdf:resource="&android-2_1;AndroidTestMockClassLibrary"/>
		<rdfs:subClassOf rdf:resource="&android-2_1;AndroidTestSuitebuilderClassLibrary"/>
		<rdfs:subClassOf rdf:resource="&android-2_1;AndroidTestSuitebuilderAnnotationClassLibrary"/>
		<rdfs:subClassOf rdf:resource="&android-2_1;JavaLangClassLibrary"/>
		<rdfs:subClassOf rdf:resource="&android-2_1;JavaLangAnnotationClassLibrary"/>
		<rdfs:subClassOf rdf:resource="&android-2_1;JavaLangReflectClassLibrary"/>
		<rdfs:subClassOf rdf:resource="&android-2_1;JavaLangRefClassLibrary"/>
		<rdfs:subClassOf rdf:resource="&android-2_1;JavaUtilClassLibrary"/>
		<rdfs:subClassOf rdf:resource="&android-2_1;JavaUtilConcurrentClassLibrary"/>
		<rdfs:subClassOf rdf:resource="&android-2_1;JavaUtilConcurrentAtomicClassLibrary"/>
		<rdfs:subClassOf rdf:resource="&android-2_1;JavaUtilConcurrentLocksClassLibrary"/>
		<rdfs:subClassOf rdf:resource="&android-2_1;JavaUtilRegexClassLibrary"/>
		<rdfs:subClassOf rdf:resource="&android-2_1;JavaUtilJarClassLibrary"/>
		<rdfs:subClassOf rdf:resource="&android-2_1;JavaUtilZipClassLibrary"/>
		<rdfs:subClassOf rdf:resource="&android-2_1;JavaUtilLoggingClassLibrary"/>
		<rdfs:subClassOf rdf:resource="&android-2_1;JavaUtilPrefsClassLibrary"/>
		<rdfs:subClassOf rdf:resource="&android-2_1;JavaIoClassLibrary"/>
		<rdfs:subClassOf rdf:resource="&android-2_1;JavaNioClassLibrary"/>
		<rdfs:subClassOf rdf:resource="&android-2_1;JavaNioChannelsClassLibrary"/>
		<rdfs:subClassOf rdf:resource="&android-2_1;JavaNioChannelsSpiClassLibrary"/>
		<rdfs:subClassOf rdf:resource="&android-2_1;JavaNioCharsetClassLibrary"/>
		<rdfs:subClassOf rdf:resource="&android-2_1;JavaNioCharsetSpiClassLibrary"/>
		<rdfs:subClassOf rdf:resource="&android-2_1;JavaNetClassLibrary"/>
		<rdfs:subClassOf rdf:resource="&android-2_1;JavaSecurityClassLibrary"/>
		<rdfs:subClassOf rdf:resource="&android-2_1;JavaSecurityCertClassLibrary"/>
		<rdfs:subClassOf rdf:resource="&android-2_1;JavaSecuritySpecClassLibrary"/>
		<rdfs:subClassOf rdf:resource="&android-2_1;JavaSecurityAclClassLibrary"/>
		<rdfs:subClassOf rdf:resource="&android-2_1;JavaSecurityInterfacesClassLibrary"/>
		<rdfs:subClassOf rdf:resource="&android-2_1;JavaTextClassLibrary"/>
		<rdfs:subClassOf rdf:resource="&android-2_1;JavaAwtFontClassLibrary"/>
		<rdfs:subClassOf rdf:resource="&android-2_1;JavaBeansClassLibrary"/>
		<rdfs:subClassOf rdf:resource="&android-2_1;JavaMathClassLibrary"/>
		<rdfs:subClassOf rdf:resource="&android-2_1;JavaSqlClassLibrary"/>
		<rdfs:subClassOf rdf:resource="&android-2_1;OrgXmlpullV1ClassLibrary"/>
		<rdfs:subClassOf rdf:resource="&android-2_1;OrgXmlpullV1Sax2ClassLibrary"/>
		<rdfs:subClassOf rdf:resource="&android-2_1;OrgXmlSaxClassLibrary"/>
		<rdfs:subClassOf rdf:resource="&android-2_1;OrgXmlSaxHelpersClassLibrary"/>
		<rdfs:subClassOf rdf:resource="&android-2_1;OrgXmlSaxExtClassLibrary"/>
		<rdfs:subClassOf rdf:resource="&android-2_1;OrgW3cDomClassLibrary"/>
		<rdfs:subClassOf rdf:resource="&android-2_1;OrgApacheCommonsLoggingClassLibrary"/>
		<rdfs:subClassOf rdf:resource="&android-2_1;OrgApacheHttpClassLibrary"/>
		<rdfs:subClassOf rdf:resource="&android-2_1;OrgApacheHttpProtocolClassLibrary"/>
		<rdfs:subClassOf rdf:resource="&android-2_1;OrgApacheHttpUtilClassLibrary"/>
		<rdfs:subClassOf rdf:resource="&android-2_1;OrgApacheHttpParamsClassLibrary"/>
		<rdfs:subClassOf rdf:resource="&android-2_1;OrgApacheHttpAuthClassLibrary"/>
		<rdfs:subClassOf rdf:resource="&android-2_1;OrgApacheHttpAuthParamsClassLibrary"/>
		<rdfs:subClassOf rdf:resource="&android-2_1;OrgApacheHttpClientClassLibrary"/>
		<rdfs:subClassOf rdf:resource="&android-2_1;OrgApacheHttpClientMethodsClassLibrary"/>
		<rdfs:subClassOf rdf:resource="&android-2_1;OrgApacheHttpClientEntityClassLibrary"/>
		<rdfs:subClassOf rdf:resource="&android-2_1;OrgApacheHttpClientParamsClassLibrary"/>
		<rdfs:subClassOf rdf:resource="&android-2_1;OrgApacheHttpClientProtocolClassLibrary"/>
		<rdfs:subClassOf rdf:resource="&android-2_1;OrgApacheHttpClientUtilsClassLibrary"/>
		<rdfs:subClassOf rdf:resource="&android-2_1;OrgApacheHttpCookieClassLibrary"/>
		<rdfs:subClassOf rdf:resource="&android-2_1;OrgApacheHttpCookieParamsClassLibrary"/>
		<rdfs:subClassOf rdf:resource="&android-2_1;OrgApacheHttpConnClassLibrary"/>
		<rdfs:subClassOf rdf:resource="&android-2_1;OrgApacheHttpConnParamsClassLibrary"/>
		<rdfs:subClassOf rdf:resource="&android-2_1;OrgApacheHttpConnSchemeClassLibrary"/>
		<rdfs:subClassOf rdf:resource="&android-2_1;OrgApacheHttpConnRoutingClassLibrary"/>
		<rdfs:subClassOf rdf:resource="&android-2_1;OrgApacheHttpConnSslClassLibrary"/>
		<rdfs:subClassOf rdf:resource="&android-2_1;OrgApacheHttpConnUtilClassLibrary"/>
		<rdfs:subClassOf rdf:resource="&android-2_1;OrgApacheHttpEntityClassLibrary"/>
		<rdfs:subClassOf rdf:resource="&android-2_1;OrgApacheHttpMessageClassLibrary"/>
		<rdfs:subClassOf rdf:resource="&android-2_1;OrgApacheHttpImplClassLibrary"/>
		<rdfs:subClassOf rdf:resource="&android-2_1;OrgApacheHttpImplEntityClassLibrary"/>
		<rdfs:subClassOf rdf:resource="&android-2_1;OrgApacheHttpImplAuthClassLibrary"/>
		<rdfs:subClassOf rdf:resource="&android-2_1;OrgApacheHttpImplClientClassLibrary"/>
		<rdfs:subClassOf rdf:resource="&android-2_1;OrgApacheHttpImplConnClassLibrary"/>
		<rdfs:subClassOf rdf:resource="&android-2_1;OrgApacheHttpImplConnTsccmClassLibrary"/>
		<rdfs:subClassOf rdf:resource="&android-2_1;OrgApacheHttpImplIoClassLibrary"/>
		<rdfs:subClassOf rdf:resource="&android-2_1;OrgApacheHttpImplCookieClassLibrary"/>
		<rdfs:subClassOf rdf:resource="&android-2_1;OrgApacheHttpIoClassLibrary"/>
		<rdfs:subClassOf rdf:resource="&android-2_1;OrgJsonClassLibrary"/>
		<rdfs:subClassOf rdf:resource="&android-2_1;JavaxMicroeditionKhronosOpenglesClassLibrary"/>
		<rdfs:subClassOf rdf:resource="&android-2_1;JavaxMicroeditionKhronosEglClassLibrary"/>
		<rdfs:subClassOf rdf:resource="&android-2_1;JavaxNetClassLibrary"/>
		<rdfs:subClassOf rdf:resource="&android-2_1;JavaxNetSslClassLibrary"/>
		<rdfs:subClassOf rdf:resource="&android-2_1;JavaxSecurityAuthClassLibrary"/>
		<rdfs:subClassOf rdf:resource="&android-2_1;JavaxSecurityAuthCallbackClassLibrary"/>
		<rdfs:subClassOf rdf:resource="&android-2_1;JavaxSecurityAuthX500ClassLibrary"/>
		<rdfs:subClassOf rdf:resource="&android-2_1;JavaxSecurityAuthLoginClassLibrary"/>
		<rdfs:subClassOf rdf:resource="&android-2_1;JavaxSecurityCertClassLibrary"/>
		<rdfs:subClassOf rdf:resource="&android-2_1;JavaxCryptoClassLibrary"/>
		<rdfs:subClassOf rdf:resource="&android-2_1;JavaxCryptoInterfacesClassLibrary"/>
		<rdfs:subClassOf rdf:resource="&android-2_1;JavaxCryptoSpecClassLibrary"/>
		<rdfs:subClassOf rdf:resource="&android-2_1;JavaxSqlClassLibrary"/>
		<rdfs:subClassOf rdf:resource="&android-2_1;JavaxXmlClassLibrary"/>
		<rdfs:subClassOf rdf:resource="&android-2_1;JavaxXmlParsersClassLibrary"/>
		<rdfs:subClassOf rdf:resource="&android-2_1;JunitFrameworkClassLibrary"/>
		<rdfs:subClassOf rdf:resource="&android-2_1;JunitRunnerClassLibrary"/>
		<rdfs:subClassOf rdf:resource="&android-2_1;DalvikAnnotationClassLibrary"/>
		<rdfs:subClassOf rdf:resource="&android-2_1;DalvikBytecodeClassLibrary"/>
		<rdfs:subClassOf rdf:resource="&android-2_1;DalvikSystemClassLibrary"/>
		<rdfs:comment xml:lang="en">Java class library implementing the Android 2.1 API</rdfs:comment>
		<rdfs:comment xml:lang="OWLManchester">platform:implementsInterface some Android2_1API</rdfs:comment>
	</owl:Class>
	<owl:Class rdf:about="&android-2_1;Android2_1BytecodeFormat">
		<owl:equivalentClass rdf:resource="&android-1_6;Android1_6BytecodeFormat"/>
		<rdfs:subClassOf rdf:resource="&isa;JavaBytecode"/>
		<rdfs:comment xml:lang="en">Android 2.1 bytecode format</rdfs:comment>
		<rdfs:comment xml:lang="OWLManchester">java:majorVersionNumber some xsd:integer[>="49"^^xsd:integer] and java:preverified value false</rdfs:comment>
	</owl:Class>
	<android-2_1:Android2_1BytecodeFormat rdf:about="&android-2_1;theAndroid2_1BytecodeFormat">
		<java:preverified rdf:datatype="http://www.w3.org/2001/XMLSchema#boolean">false</java:preverified>
		<java:minorVersionNumber rdf:datatype="http://www.w3.org/2001/XMLSchema#integer">0</java:minorVersionNumber>
		<java:majorVersionNumber rdf:datatype="http://www.w3.org/2001/XMLSchema#integer">49</java:majorVersionNumber>
	</android-2_1:Android2_1BytecodeFormat>
	<android-2_1:Android2_1API rdf:about="&android-2_1;theAndroid2_1API">
		<platform:comprisesInterfacePart rdf:resource="&android-2_1;theDalvikSystemPart"/>
		<platform:comprisesInterfacePart rdf:resource="&android-2_1;theDalvikBytecodePart"/>
		<platform:comprisesInterfacePart rdf:resource="&android-2_1;theDalvikAnnotationPart"/>
		<platform:comprisesInterfacePart rdf:resource="&android-2_1;theJunitRunnerPart"/>
		<platform:comprisesInterfacePart rdf:resource="&android-2_1;theJunitFrameworkPart"/>
		<platform:comprisesInterfacePart rdf:resource="&android-2_1;theJavaxXmlParsersPart"/>
		<platform:comprisesInterfacePart rdf:resource="&android-2_1;theJavaxXmlPart"/>
		<platform:comprisesInterfacePart rdf:resource="&android-2_1;theJavaxSqlPart"/>
		<platform:comprisesInterfacePart rdf:resource="&android-2_1;theJavaxCryptoSpecPart"/>
		<platform:comprisesInterfacePart rdf:resource="&android-2_1;theJavaxCryptoInterfacesPart"/>
		<platform:comprisesInterfacePart rdf:resource="&android-2_1;theJavaxCryptoPart"/>
		<platform:comprisesInterfacePart rdf:resource="&android-2_1;theJavaxSecurityCertPart"/>
		<platform:comprisesInterfacePart rdf:resource="&android-2_1;theJavaxSecurityAuthLoginPart"/>
		<platform:comprisesInterfacePart rdf:resource="&android-2_1;theJavaxSecurityAuthX500Part"/>
		<platform:comprisesInterfacePart rdf:resource="&android-2_1;theJavaxSecurityAuthCallbackPart"/>
		<platform:comprisesInterfacePart rdf:resource="&android-2_1;theJavaxSecurityAuthPart"/>
		<platform:comprisesInterfacePart rdf:resource="&android-2_1;theJavaxNetSslPart"/>
		<platform:comprisesInterfacePart rdf:resource="&android-2_1;theJavaxNetPart"/>
		<platform:comprisesInterfacePart rdf:resource="&android-2_1;theJavaxMicroeditionKhronosEglPart"/>
		<platform:comprisesInterfacePart rdf:resource="&android-2_1;theJavaxMicroeditionKhronosOpenglesPart"/>
		<platform:comprisesInterfacePart rdf:resource="&android-2_1;theOrgJsonPart"/>
		<platform:comprisesInterfacePart rdf:resource="&android-2_1;theOrgApacheHttpIoPart"/>
		<platform:comprisesInterfacePart rdf:resource="&android-2_1;theOrgApacheHttpImplCookiePart"/>
		<platform:comprisesInterfacePart rdf:resource="&android-2_1;theOrgApacheHttpImplIoPart"/>
		<platform:comprisesInterfacePart rdf:resource="&android-2_1;theOrgApacheHttpImplConnTsccmPart"/>
		<platform:comprisesInterfacePart rdf:resource="&android-2_1;theOrgApacheHttpImplConnPart"/>
		<platform:comprisesInterfacePart rdf:resource="&android-2_1;theOrgApacheHttpImplClientPart"/>
		<platform:comprisesInterfacePart rdf:resource="&android-2_1;theOrgApacheHttpImplAuthPart"/>
		<platform:comprisesInterfacePart rdf:resource="&android-2_1;theOrgApacheHttpImplEntityPart"/>
		<platform:comprisesInterfacePart rdf:resource="&android-2_1;theOrgApacheHttpImplPart"/>
		<platform:comprisesInterfacePart rdf:resource="&android-2_1;theOrgApacheHttpMessagePart"/>
		<platform:comprisesInterfacePart rdf:resource="&android-2_1;theOrgApacheHttpEntityPart"/>
		<platform:comprisesInterfacePart rdf:resource="&android-2_1;theOrgApacheHttpConnUtilPart"/>
		<platform:comprisesInterfacePart rdf:resource="&android-2_1;theOrgApacheHttpConnSslPart"/>
		<platform:comprisesInterfacePart rdf:resource="&android-2_1;theOrgApacheHttpConnRoutingPart"/>
		<platform:comprisesInterfacePart rdf:resource="&android-2_1;theOrgApacheHttpConnSchemePart"/>
		<platform:comprisesInterfacePart rdf:resource="&android-2_1;theOrgApacheHttpConnParamsPart"/>
		<platform:comprisesInterfacePart rdf:resource="&android-2_1;theOrgApacheHttpConnPart"/>
		<platform:comprisesInterfacePart rdf:resource="&android-2_1;theOrgApacheHttpCookieParamsPart"/>
		<platform:comprisesInterfacePart rdf:resource="&android-2_1;theOrgApacheHttpCookiePart"/>
		<platform:comprisesInterfacePart rdf:resource="&android-2_1;theOrgApacheHttpClientUtilsPart"/>
		<platform:comprisesInterfacePart rdf:resource="&android-2_1;theOrgApacheHttpClientProtocolPart"/>
		<platform:comprisesInterfacePart rdf:resource="&android-2_1;theOrgApacheHttpClientParamsPart"/>
		<platform:comprisesInterfacePart rdf:resource="&android-2_1;theOrgApacheHttpClientEntityPart"/>
		<platform:comprisesInterfacePart rdf:resource="&android-2_1;theOrgApacheHttpClientMethodsPart"/>
		<platform:comprisesInterfacePart rdf:resource="&android-2_1;theOrgApacheHttpClientPart"/>
		<platform:comprisesInterfacePart rdf:resource="&android-2_1;theOrgApacheHttpAuthParamsPart"/>
		<platform:comprisesInterfacePart rdf:resource="&android-2_1;theOrgApacheHttpAuthPart"/>
		<platform:comprisesInterfacePart rdf:resource="&android-2_1;theOrgApacheHttpParamsPart"/>
		<platform:comprisesInterfacePart rdf:resource="&android-2_1;theOrgApacheHttpUtilPart"/>
		<platform:comprisesInterfacePart rdf:resource="&android-2_1;theOrgApacheHttpProtocolPart"/>
		<platform:comprisesInterfacePart rdf:resource="&android-2_1;theOrgApacheHttpPart"/>
		<platform:comprisesInterfacePart rdf:resource="&android-2_1;theOrgApacheCommonsLoggingPart"/>
		<platform:comprisesInterfacePart rdf:resource="&android-2_1;theOrgW3cDomPart"/>
		<platform:comprisesInterfacePart rdf:resource="&android-2_1;theOrgXmlSaxExtPart"/>
		<platform:comprisesInterfacePart rdf:resource="&android-2_1;theOrgXmlSaxHelpersPart"/>
		<platform:comprisesInterfacePart rdf:resource="&android-2_1;theOrgXmlSaxPart"/>
		<platform:comprisesInterfacePart rdf:resource="&android-2_1;theOrgXmlpullV1Sax2Part"/>
		<platform:comprisesInterfacePart rdf:resource="&android-2_1;theOrgXmlpullV1Part"/>
		<platform:comprisesInterfacePart rdf:resource="&android-2_1;theJavaSqlPart"/>
		<platform:comprisesInterfacePart rdf:resource="&android-2_1;theJavaMathPart"/>
		<platform:comprisesInterfacePart rdf:resource="&android-2_1;theJavaBeansPart"/>
		<platform:comprisesInterfacePart rdf:resource="&android-2_1;theJavaAwtFontPart"/>
		<platform:comprisesInterfacePart rdf:resource="&android-2_1;theJavaTextPart"/>
		<platform:comprisesInterfacePart rdf:resource="&android-2_1;theJavaSecurityInterfacesPart"/>
		<platform:comprisesInterfacePart rdf:resource="&android-2_1;theJavaSecurityAclPart"/>
		<platform:comprisesInterfacePart rdf:resource="&android-2_1;theJavaSecuritySpecPart"/>
		<platform:comprisesInterfacePart rdf:resource="&android-2_1;theJavaSecurityCertPart"/>
		<platform:comprisesInterfacePart rdf:resource="&android-2_1;theJavaSecurityPart"/>
		<platform:comprisesInterfacePart rdf:resource="&android-2_1;theJavaNetPart"/>
		<platform:comprisesInterfacePart rdf:resource="&android-2_1;theJavaNioCharsetSpiPart"/>
		<platform:comprisesInterfacePart rdf:resource="&android-2_1;theJavaNioCharsetPart"/>
		<platform:comprisesInterfacePart rdf:resource="&android-2_1;theJavaNioChannelsSpiPart"/>
		<platform:comprisesInterfacePart rdf:resource="&android-2_1;theJavaNioChannelsPart"/>
		<platform:comprisesInterfacePart rdf:resource="&android-2_1;theJavaNioPart"/>
		<platform:comprisesInterfacePart rdf:resource="&android-2_1;theJavaIoPart"/>
		<platform:comprisesInterfacePart rdf:resource="&android-2_1;theJavaUtilPrefsPart"/>
		<platform:comprisesInterfacePart rdf:resource="&android-2_1;theJavaUtilLoggingPart"/>
		<platform:comprisesInterfacePart rdf:resource="&android-2_1;theJavaUtilZipPart"/>
		<platform:comprisesInterfacePart rdf:resource="&android-2_1;theJavaUtilJarPart"/>
		<platform:comprisesInterfacePart rdf:resource="&android-2_1;theJavaUtilRegexPart"/>
		<platform:comprisesInterfacePart rdf:resource="&android-2_1;theJavaUtilConcurrentLocksPart"/>
		<platform:comprisesInterfacePart rdf:resource="&android-2_1;theJavaUtilConcurrentAtomicPart"/>
		<platform:comprisesInterfacePart rdf:resource="&android-2_1;theJavaUtilConcurrentPart"/>
		<platform:comprisesInterfacePart rdf:resource="&android-2_1;theJavaUtilPart"/>
		<platform:comprisesInterfacePart rdf:resource="&android-2_1;theJavaLangRefPart"/>
		<platform:comprisesInterfacePart rdf:resource="&android-2_1;theJavaLangReflectPart"/>
		<platform:comprisesInterfacePart rdf:resource="&android-2_1;theJavaLangAnnotationPart"/>
		<platform:comprisesInterfacePart rdf:resource="&android-2_1;theJavaLangPart"/>
		<platform:comprisesInterfacePart rdf:resource="&android-2_1;theAndroidTestSuitebuilderAnnotationPart"/>
		<platform:comprisesInterfacePart rdf:resource="&android-2_1;theAndroidTestSuitebuilderPart"/>
		<platform:comprisesInterfacePart rdf:resource="&android-2_1;theAndroidTestMockPart"/>
		<platform:comprisesInterfacePart rdf:resource="&android-2_1;theAndroidTestPart"/>
		<platform:comprisesInterfacePart rdf:resource="&android-2_1;theAndroidTextUtilPart"/>
		<platform:comprisesInterfacePart rdf:resource="&android-2_1;theAndroidTextStylePart"/>
		<platform:comprisesInterfacePart rdf:resource="&android-2_1;theAndroidTextMethodPart"/>
		<platform:comprisesInterfacePart rdf:resource="&android-2_1;theAndroidTextFormatPart"/>
		<platform:comprisesInterfacePart rdf:resource="&android-2_1;theAndroidTextPart"/>
		<platform:comprisesInterfacePart rdf:resource="&android-2_1;theAndroidTelephonyGsmPart"/>
		<platform:comprisesInterfacePart rdf:resource="&android-2_1;theAndroidTelephonyCdmaPart"/>
		<platform:comprisesInterfacePart rdf:resource="&android-2_1;theAndroidTelephonyPart"/>
		<platform:comprisesInterfacePart rdf:resource="&android-2_1;theAndroidSpeechTtsPart"/>
		<platform:comprisesInterfacePart rdf:resource="&android-2_1;theAndroidSpeechPart"/>
		<platform:comprisesInterfacePart rdf:resource="&android-2_1;theAndroidServiceWallpaperPart"/>
		<platform:comprisesInterfacePart rdf:resource="&android-2_1;theAndroidSaxPart"/>
		<platform:comprisesInterfacePart rdf:resource="&android-2_1;theAndroidWebkitPart"/>
		<platform:comprisesInterfacePart rdf:resource="&android-2_1;theAndroidProviderPart"/>
		<platform:comprisesInterfacePart rdf:resource="&android-2_1;theAndroidPreferencePart"/>
		<platform:comprisesInterfacePart rdf:resource="&android-2_1;theAndroidOpenglPart"/>
		<platform:comprisesInterfacePart rdf:resource="&android-2_1;theAndroidMediaPart"/>
		<platform:comprisesInterfacePart rdf:resource="&android-2_1;theAndroidLocationPart"/>
		<platform:comprisesInterfacePart rdf:resource="&android-2_1;theAndroidInputmethodservicePart"/>
		<platform:comprisesInterfacePart rdf:resource="&android-2_1;theAndroidHardwarePart"/>
		<platform:comprisesInterfacePart rdf:resource="&android-2_1;theAndroidGesturePart"/>
		<platform:comprisesInterfacePart rdf:resource="&android-2_1;theAndroidBluetoothPart"/>
		<platform:comprisesInterfacePart rdf:resource="&android-2_1;theAndroidAppwidgetPart"/>
		<platform:comprisesInterfacePart rdf:resource="&android-2_1;theAndroidWidgetPart"/>
		<platform:comprisesInterfacePart rdf:resource="&android-2_1;theAndroidUtilPart"/>
		<platform:comprisesInterfacePart rdf:resource="&android-2_1;theAndroidDatabaseSqlitePart"/>
		<platform:comprisesInterfacePart rdf:resource="&android-2_1;theAndroidDatabasePart"/>
		<platform:comprisesInterfacePart rdf:resource="&android-2_1;theAndroidNetWifiPart"/>
		<platform:comprisesInterfacePart rdf:resource="&android-2_1;theAndroidNetHttpPart"/>
		<platform:comprisesInterfacePart rdf:resource="&android-2_1;theAndroidNetPart"/>
		<platform:comprisesInterfacePart rdf:resource="&android-2_1;theAndroidGraphicsDrawableShapesPart"/>
		<platform:comprisesInterfacePart rdf:resource="&android-2_1;theAndroidGraphicsDrawablePart"/>
		<platform:comprisesInterfacePart rdf:resource="&android-2_1;theAndroidGraphicsPart"/>
		<platform:comprisesInterfacePart rdf:resource="&android-2_1;theAndroidAccountsPart"/>
		<platform:comprisesInterfacePart rdf:resource="&android-2_1;theAndroidOsPart"/>
		<platform:comprisesInterfacePart rdf:resource="&android-2_1;theAndroidContentPmPart"/>
		<platform:comprisesInterfacePart rdf:resource="&android-2_1;theAndroidContentResPart"/>
		<platform:comprisesInterfacePart rdf:resource="&android-2_1;theAndroidContentPart"/>
		<platform:comprisesInterfacePart rdf:resource="&android-2_1;theAndroidViewAnimationPart"/>
		<platform:comprisesInterfacePart rdf:resource="&android-2_1;theAndroidViewInputmethodPart"/>
		<platform:comprisesInterfacePart rdf:resource="&android-2_1;theAndroidViewAccessibilityPart"/>
		<platform:comprisesInterfacePart rdf:resource="&android-2_1;theAndroidViewPart"/>
		<platform:comprisesInterfacePart rdf:resource="&android-2_1;theAndroidAppPart"/>
		<platform:comprisesInterfacePart rdf:resource="&android-2_1;theAndroidAccessibilityservicePart"/>
		<platform:comprisesInterfacePart rdf:resource="&android-2_1;theAndroidPart"/>
	</android-2_1:Android2_1API>
	<owl:Class rdf:about="&android-2_1;Android2_1VM">
		<owl:equivalentClass>
			<owl:Restriction>
				<owl:onProperty rdf:resource="&platform;implementsInterface"/>
				<owl:someValuesFrom rdf:resource="&android-2_1;Android2_1BytecodeFormat"/>
			</owl:Restriction>
		</owl:equivalentClass>
		<rdfs:subClassOf rdf:resource="&java;JavaVM"/>
		<rdfs:comment xml:lang="en">Android 2.1 virtual machine</rdfs:comment>
	</owl:Class>
	<owl:Class rdf:about="&android-2_1;Android2_1JRE">
		<owl:equivalentClass>
			<owl:Class >
				<owl:intersectionOf rdf:parseType="Collection">
					<owl:Restriction>
						<owl:onProperty rdf:resource="&platform;providesFeature"/>
						<owl:someValuesFrom rdf:resource="&android-2_1;Android2_1ClassLibrary"/>
					</owl:Restriction>
					<owl:Restriction>
						<owl:onProperty rdf:resource="&platform;providesFeature"/>
						<owl:someValuesFrom rdf:resource="&android-2_1;Android2_1VM"/>
					</owl:Restriction>
				</owl:intersectionOf>
			</owl:Class>
		</owl:equivalentClass>
		<rdfs:subClassOf rdf:resource="&java;JRE"/>
		<rdfs:comment xml:lang="en">Android 2.1 Java Runtime Environment</rdfs:comment>
	</owl:Class>
	<owl:Class rdf:about="&android-2_1;Android">
		<rdfs:subClassOf rdf:resource="&android-1_6;Android"/>
		<rdfs:seeAlso rdf:resource="&android-2_1;JavaLang"/>
		<rdfs:comment xml:lang="en">Java API part implementing the android package for Android 2.1</rdfs:comment>
	</owl:Class>
	<owl:Class rdf:about="&android-2_1;AndroidAccessibilityservice">
		<rdfs:subClassOf rdf:resource="&android-1_6;AndroidAccessibilityservice"/>
		<rdfs:seeAlso rdf:resource="&android-2_1;AndroidApp"/>
		<rdfs:seeAlso rdf:resource="&android-2_1;AndroidContent"/>
		<rdfs:seeAlso rdf:resource="&android-2_1;JavaLang"/>
		<rdfs:seeAlso rdf:resource="&android-2_1;AndroidOs"/>
		<rdfs:seeAlso rdf:resource="&android-2_1;AndroidViewAccessibility"/>
		<rdfs:comment xml:lang="en">Java API part implementing the android.accessibilityservice package for Android 2.1</rdfs:comment>
	</owl:Class>
	<owl:Class rdf:about="&android-2_1;AndroidApp">
		<rdfs:subClassOf rdf:resource="&android-1_6;AndroidApp"/>
		<rdfs:seeAlso rdf:resource="&android-2_1;AndroidContentPm"/>
		<rdfs:seeAlso rdf:resource="&android-2_1;JavaLang"/>
		<rdfs:seeAlso rdf:resource="&android-2_1;AndroidViewAccessibility"/>
		<rdfs:seeAlso rdf:resource="&android-2_1;AndroidNet"/>
		<rdfs:seeAlso rdf:resource="&android-2_1;AndroidView"/>
		<rdfs:seeAlso rdf:resource="&android-2_1;AndroidContentRes"/>
		<rdfs:seeAlso rdf:resource="&android-2_1;AndroidUtil"/>
		<rdfs:seeAlso rdf:resource="&android-2_1;AndroidOs"/>
		<rdfs:seeAlso rdf:resource="&android-2_1;AndroidDatabase"/>
		<rdfs:seeAlso rdf:resource="&android-2_1;AndroidGraphics"/>
		<rdfs:seeAlso rdf:resource="&android-2_1;AndroidContent"/>
		<rdfs:seeAlso rdf:resource="&android-2_1;AndroidWidget"/>
		<rdfs:seeAlso rdf:resource="&android-2_1;AndroidGraphicsDrawable"/>
		<rdfs:seeAlso rdf:resource="&android-2_1;JavaUtil"/>
		<rdfs:seeAlso rdf:resource="&android-2_1;JavaIo"/>
		<rdfs:comment xml:lang="en">Java API part implementing the android.app package for Android 2.1</rdfs:comment>
	</owl:Class>
	<owl:Class rdf:about="&android-2_1;AndroidView">
		<rdfs:subClassOf rdf:resource="&java;JavaAPIPart"/>
		<rdfs:seeAlso rdf:resource="&android-2_1;JavaLangAnnotation"/>
		<rdfs:seeAlso rdf:resource="&android-2_1;AndroidGraphics"/>
		<rdfs:seeAlso rdf:resource="&android-2_1;AndroidContent"/>
		<rdfs:seeAlso rdf:resource="&android-2_1;JavaLang"/>
		<rdfs:seeAlso rdf:resource="&android-2_1;AndroidViewAnimation"/>
		<rdfs:seeAlso rdf:resource="&android-2_1;AndroidGraphicsDrawable"/>
		<rdfs:seeAlso rdf:resource="&android-2_1;AndroidViewAccessibility"/>
		<rdfs:seeAlso rdf:resource="&android-2_1;AndroidNet"/>
		<rdfs:seeAlso rdf:resource="&android-2_1;JavaUtil"/>
		<rdfs:seeAlso rdf:resource="&android-2_1;OrgXmlpullV1"/>
		<rdfs:seeAlso rdf:resource="&android-2_1;AndroidViewInputmethod"/>
		<rdfs:seeAlso rdf:resource="&android-2_1;AndroidContentRes"/>
		<rdfs:seeAlso rdf:resource="&android-2_1;AndroidUtil"/>
		<rdfs:seeAlso rdf:resource="&android-2_1;AndroidOs"/>
		<rdfs:seeAlso rdf:resource="&android-2_1;AndroidHardware"/>
		<rdfs:comment xml:lang="en">Java API part implementing the android.view package for Android 2.1</rdfs:comment>
	</owl:Class>
	<owl:Class rdf:about="&android-2_1;AndroidViewAccessibility">
		<owl:equivalentClass rdf:resource="&android-1_6;AndroidViewAccessibility"/>
		<rdfs:subClassOf rdf:resource="&java;JavaAPIPart"/>
		<rdfs:seeAlso rdf:resource="&android-2_1;JavaLang"/>
		<rdfs:seeAlso rdf:resource="&android-2_1;AndroidOs"/>
		<rdfs:seeAlso rdf:resource="&android-2_1;JavaUtil"/>
		<rdfs:comment xml:lang="en">Java API part implementing the android.view.accessibility package for Android 2.1</rdfs:comment>
	</owl:Class>
	<owl:Class rdf:about="&android-2_1;AndroidViewInputmethod">
		<rdfs:subClassOf rdf:resource="&android-1_6;AndroidViewInputmethod"/>
		<rdfs:seeAlso rdf:resource="&android-2_1;AndroidGraphics"/>
		<rdfs:seeAlso rdf:resource="&android-2_1;AndroidContent"/>
		<rdfs:seeAlso rdf:resource="&android-2_1;AndroidContentPm"/>
		<rdfs:seeAlso rdf:resource="&android-2_1;JavaLang"/>
		<rdfs:seeAlso rdf:resource="&android-2_1;AndroidGraphicsDrawable"/>
		<rdfs:seeAlso rdf:resource="&android-2_1;AndroidView"/>
		<rdfs:seeAlso rdf:resource="&android-2_1;JavaUtil"/>
		<rdfs:seeAlso rdf:resource="&android-2_1;AndroidText"/>
		<rdfs:seeAlso rdf:resource="&android-2_1;AndroidUtil"/>
		<rdfs:seeAlso rdf:resource="&android-2_1;AndroidOs"/>
		<rdfs:comment xml:lang="en">Java API part implementing the android.view.inputmethod package for Android 2.1</rdfs:comment>
	</owl:Class>
	<owl:Class rdf:about="&android-2_1;AndroidViewAnimation">
		<rdfs:subClassOf rdf:resource="&android-1_6;AndroidViewAnimation"/>
		<rdfs:seeAlso rdf:resource="&android-2_1;AndroidGraphics"/>
		<rdfs:seeAlso rdf:resource="&android-2_1;AndroidContent"/>
		<rdfs:seeAlso rdf:resource="&android-2_1;AndroidUtil"/>
		<rdfs:seeAlso rdf:resource="&android-2_1;AndroidView"/>
		<rdfs:seeAlso rdf:resource="&android-2_1;JavaLang"/>
		<rdfs:seeAlso rdf:resource="&android-2_1;JavaUtil"/>
		<rdfs:comment xml:lang="en">Java API part implementing the android.view.animation package for Android 2.1</rdfs:comment>
	</owl:Class>
	<owl:Class rdf:about="&android-2_1;AndroidContent">
		<rdfs:subClassOf rdf:resource="&android-1_6;AndroidContent"/>
		<rdfs:seeAlso rdf:resource="&android-2_1;AndroidContentPm"/>
		<rdfs:seeAlso rdf:resource="&android-2_1;JavaLang"/>
		<rdfs:seeAlso rdf:resource="&android-2_1;AndroidNet"/>
		<rdfs:seeAlso rdf:resource="&android-2_1;AndroidView"/>
		<rdfs:seeAlso rdf:resource="&android-2_1;OrgXmlpullV1"/>
		<rdfs:seeAlso rdf:resource="&android-2_1;AndroidContentRes"/>
		<rdfs:seeAlso rdf:resource="&android-2_1;AndroidUtil"/>
		<rdfs:seeAlso rdf:resource="&android-2_1;AndroidOs"/>
		<rdfs:seeAlso rdf:resource="&android-2_1;AndroidDatabase"/>
		<rdfs:seeAlso rdf:resource="&android-2_1;AndroidGraphics"/>
		<rdfs:seeAlso rdf:resource="&android-2_1;AndroidGraphicsDrawable"/>
		<rdfs:seeAlso rdf:resource="&android-2_1;JavaUtil"/>
		<rdfs:seeAlso rdf:resource="&android-2_1;JavaIo"/>
		<rdfs:seeAlso rdf:resource="&android-2_1;AndroidDatabaseSqlite"/>
		<rdfs:seeAlso rdf:resource="&android-2_1;AndroidAccounts"/>
		<rdfs:comment xml:lang="en">Java API part implementing the android.content package for Android 2.1</rdfs:comment>
	</owl:Class>
	<owl:Class rdf:about="&android-2_1;AndroidContentRes">
		<rdfs:subClassOf rdf:resource="&android-1_6;AndroidContentRes"/>
		<rdfs:seeAlso rdf:resource="&android-2_1;AndroidGraphics"/>
		<rdfs:seeAlso rdf:resource="&android-2_1;JavaLang"/>
		<rdfs:seeAlso rdf:resource="&android-2_1;OrgXmlpullV1"/>
		<rdfs:seeAlso rdf:resource="&android-2_1;JavaUtil"/>
		<rdfs:seeAlso rdf:resource="&android-2_1;JavaIo"/>
		<rdfs:seeAlso rdf:resource="&android-2_1;AndroidUtil"/>
		<rdfs:seeAlso rdf:resource="&android-2_1;AndroidOs"/>
		<rdfs:seeAlso rdf:resource="&android-2_1;AndroidGraphicsDrawable"/>
		<rdfs:comment xml:lang="en">Java API part implementing the android.content.res package for Android 2.1</rdfs:comment>
	</owl:Class>
	<owl:Class rdf:about="&android-2_1;AndroidContentPm">
		<rdfs:subClassOf rdf:resource="&android-1_6;AndroidContentPm"/>
		<rdfs:seeAlso rdf:resource="&android-2_1;AndroidContent"/>
		<rdfs:seeAlso rdf:resource="&android-2_1;JavaLang"/>
		<rdfs:seeAlso rdf:resource="&android-2_1;JavaUtil"/>
		<rdfs:seeAlso rdf:resource="&android-2_1;AndroidContentRes"/>
		<rdfs:seeAlso rdf:resource="&android-2_1;AndroidUtil"/>
		<rdfs:seeAlso rdf:resource="&android-2_1;AndroidOs"/>
		<rdfs:seeAlso rdf:resource="&android-2_1;AndroidGraphicsDrawable"/>
		<rdfs:comment xml:lang="en">Java API part implementing the android.content.pm package for Android 2.1</rdfs:comment>
	</owl:Class>
	<owl:Class rdf:about="&android-2_1;AndroidOs">
		<rdfs:subClassOf rdf:resource="&android-1_6;AndroidOs"/>
		<rdfs:seeAlso rdf:resource="&android-2_1;JavaLang"/>
		<rdfs:seeAlso rdf:resource="&android-2_1;JavaNet"/>
		<rdfs:seeAlso rdf:resource="&android-2_1;JavaUtilConcurrent"/>
		<rdfs:seeAlso rdf:resource="&android-2_1;JavaUtil"/>
		<rdfs:seeAlso rdf:resource="&android-2_1;JavaIo"/>
		<rdfs:seeAlso rdf:resource="&android-2_1;AndroidUtil"/>
		<rdfs:comment xml:lang="en">Java API part implementing the android.os package for Android 2.1</rdfs:comment>
	</owl:Class>
	<owl:Class rdf:about="&android-2_1;AndroidAccounts">
		<rdfs:subClassOf rdf:resource="&java;JavaAPIPart"/>
		<rdfs:seeAlso rdf:resource="&android-2_1;AndroidContent"/>
		<rdfs:seeAlso rdf:resource="&android-2_1;JavaLang"/>
		<rdfs:seeAlso rdf:resource="&android-2_1;AndroidApp"/>
		<rdfs:seeAlso rdf:resource="&android-2_1;AndroidOs"/>
		<rdfs:seeAlso rdf:resource="&android-2_1;JavaUtilConcurrent"/>
		<rdfs:comment xml:lang="en">Java API part implementing the android.accounts package for Android 2.1</rdfs:comment>
	</owl:Class>
	<owl:Class rdf:about="&android-2_1;AndroidGraphics">
		<rdfs:subClassOf rdf:resource="&android-1_6;AndroidGraphics"/>
		<rdfs:seeAlso rdf:resource="&android-2_1;JavaLang"/>
		<rdfs:seeAlso rdf:resource="&android-2_1;JavaxMicroeditionKhronosOpengles"/>
		<rdfs:seeAlso rdf:resource="&android-2_1;AndroidContentRes"/>
		<rdfs:seeAlso rdf:resource="&android-2_1;JavaIo"/>
		<rdfs:seeAlso rdf:resource="&android-2_1;AndroidUtil"/>
		<rdfs:seeAlso rdf:resource="&android-2_1;AndroidOs"/>
		<rdfs:seeAlso rdf:resource="&android-2_1;JavaNio"/>
		<rdfs:comment xml:lang="en">Java API part implementing the android.graphics package for Android 2.1</rdfs:comment>
	</owl:Class>
	<owl:Class rdf:about="&android-2_1;AndroidGraphicsDrawable">
		<rdfs:subClassOf rdf:resource="&android-1_6;AndroidGraphicsDrawable"/>
		<rdfs:seeAlso rdf:resource="&android-2_1;AndroidGraphicsDrawableShapes"/>
		<rdfs:seeAlso rdf:resource="&android-2_1;AndroidGraphics"/>
		<rdfs:seeAlso rdf:resource="&android-2_1;JavaLang"/>
		<rdfs:seeAlso rdf:resource="&android-2_1;OrgXmlpullV1"/>
		<rdfs:seeAlso rdf:resource="&android-2_1;AndroidContentRes"/>
		<rdfs:seeAlso rdf:resource="&android-2_1;JavaIo"/>
		<rdfs:seeAlso rdf:resource="&android-2_1;AndroidUtil"/>
		<rdfs:comment xml:lang="en">Java API part implementing the android.graphics.drawable package for Android 2.1</rdfs:comment>
	</owl:Class>
	<owl:Class rdf:about="&android-2_1;AndroidGraphicsDrawableShapes">
		<owl:equivalentClass rdf:resource="&android-1_6;AndroidGraphicsDrawableShapes"/>
		<rdfs:subClassOf rdf:resource="&java;JavaAPIPart"/>
		<rdfs:seeAlso rdf:resource="&android-2_1;AndroidGraphics"/>
		<rdfs:seeAlso rdf:resource="&android-2_1;JavaLang"/>
		<rdfs:comment xml:lang="en">Java API part implementing the android.graphics.drawable.shapes package for Android 2.1</rdfs:comment>
	</owl:Class>
	<owl:Class rdf:about="&android-2_1;AndroidNet">
		<owl:equivalentClass rdf:resource="&android-1_6;AndroidNet"/>
		<rdfs:subClassOf rdf:resource="&java;JavaAPIPart"/>
		<rdfs:seeAlso rdf:resource="&android-2_1;JavaxNet"/>
		<rdfs:seeAlso rdf:resource="&android-2_1;AndroidContent"/>
		<rdfs:seeAlso rdf:resource="&android-2_1;JavaLang"/>
		<rdfs:seeAlso rdf:resource="&android-2_1;JavaUtil"/>
		<rdfs:seeAlso rdf:resource="&android-2_1;JavaIo"/>
		<rdfs:seeAlso rdf:resource="&android-2_1;JavaxNetSsl"/>
		<rdfs:seeAlso rdf:resource="&android-2_1;AndroidOs"/>
		<rdfs:seeAlso rdf:resource="&android-2_1;JavaNet"/>
		<rdfs:comment xml:lang="en">Java API part implementing the android.net package for Android 2.1</rdfs:comment>
	</owl:Class>
	<owl:Class rdf:about="&android-2_1;AndroidNetHttp">
		<owl:equivalentClass rdf:resource="&android-1_6;AndroidNetHttp"/>
		<rdfs:subClassOf rdf:resource="&java;JavaAPIPart"/>
		<rdfs:seeAlso rdf:resource="&android-2_1;JavaSecurityCert"/>
		<rdfs:seeAlso rdf:resource="&android-2_1;JavaLang"/>
		<rdfs:seeAlso rdf:resource="&android-2_1;AndroidOs"/>
		<rdfs:comment xml:lang="en">Java API part implementing the android.net.http package for Android 2.1</rdfs:comment>
	</owl:Class>
	<owl:Class rdf:about="&android-2_1;AndroidNetWifi">
		<owl:equivalentClass rdf:resource="&android-1_6;AndroidNetWifi"/>
		<rdfs:subClassOf rdf:resource="&java;JavaAPIPart"/>
		<rdfs:seeAlso rdf:resource="&android-2_1;AndroidNet"/>
		<rdfs:seeAlso rdf:resource="&android-2_1;JavaLang"/>
		<rdfs:seeAlso rdf:resource="&android-2_1;AndroidOs"/>
		<rdfs:seeAlso rdf:resource="&android-2_1;JavaUtil"/>
		<rdfs:comment xml:lang="en">Java API part implementing the android.net.wifi package for Android 2.1</rdfs:comment>
	</owl:Class>
	<owl:Class rdf:about="&android-2_1;AndroidDatabase">
		<rdfs:subClassOf rdf:resource="&android-1_6;AndroidDatabase"/>
		<rdfs:seeAlso rdf:resource="&android-2_1;AndroidContent"/>
		<rdfs:seeAlso rdf:resource="&android-2_1;JavaLang"/>
		<rdfs:seeAlso rdf:resource="&android-2_1;AndroidNet"/>
		<rdfs:seeAlso rdf:resource="&android-2_1;JavaUtil"/>
		<rdfs:seeAlso rdf:resource="&android-2_1;JavaIo"/>
		<rdfs:seeAlso rdf:resource="&android-2_1;AndroidDatabaseSqlite"/>
		<rdfs:seeAlso rdf:resource="&android-2_1;AndroidOs"/>
		<rdfs:comment xml:lang="en">Java API part implementing the android.database package for Android 2.1</rdfs:comment>
	</owl:Class>
	<owl:Class rdf:about="&android-2_1;AndroidDatabaseSqlite">
		<rdfs:subClassOf rdf:resource="&android-1_6;AndroidDatabaseSqlite"/>
		<rdfs:seeAlso rdf:resource="&android-2_1;AndroidDatabase"/>
		<rdfs:seeAlso rdf:resource="&android-2_1;AndroidContent"/>
		<rdfs:seeAlso rdf:resource="&android-2_1;JavaLang"/>
		<rdfs:seeAlso rdf:resource="&android-2_1;JavaUtil"/>
		<rdfs:seeAlso rdf:resource="&android-2_1;JavaIo"/>
		<rdfs:comment xml:lang="en">Java API part implementing the android.database.sqlite package for Android 2.1</rdfs:comment>
	</owl:Class>
	<owl:Class rdf:about="&android-2_1;AndroidUtil">
		<rdfs:subClassOf rdf:resource="&android-1_6;AndroidUtil"/>
		<rdfs:seeAlso rdf:resource="&android-2_1;OrgXmlSax"/>
		<rdfs:seeAlso rdf:resource="&android-2_1;JavaLang"/>
		<rdfs:seeAlso rdf:resource="&android-2_1;JavaUtil"/>
		<rdfs:seeAlso rdf:resource="&android-2_1;OrgXmlpullV1"/>
		<rdfs:seeAlso rdf:resource="&android-2_1;JavaIo"/>
		<rdfs:comment xml:lang="en">Java API part implementing the android.util package for Android 2.1</rdfs:comment>
	</owl:Class>
	<owl:Class rdf:about="&android-2_1;AndroidWidget">
		<rdfs:subClassOf rdf:resource="&java;JavaAPIPart"/>
		<rdfs:seeAlso rdf:resource="&android-2_1;JavaLang"/>
		<rdfs:seeAlso rdf:resource="&android-2_1;AndroidViewAnimation"/>
		<rdfs:seeAlso rdf:resource="&android-2_1;AndroidViewAccessibility"/>
		<rdfs:seeAlso rdf:resource="&android-2_1;AndroidNet"/>
		<rdfs:seeAlso rdf:resource="&android-2_1;AndroidView"/>
		<rdfs:seeAlso rdf:resource="&android-2_1;AndroidText"/>
		<rdfs:seeAlso rdf:resource="&android-2_1;AndroidContentRes"/>
		<rdfs:seeAlso rdf:resource="&android-2_1;AndroidUtil"/>
		<rdfs:seeAlso rdf:resource="&android-2_1;AndroidOs"/>
		<rdfs:seeAlso rdf:resource="&android-2_1;JavaLangAnnotation"/>
		<rdfs:seeAlso rdf:resource="&android-2_1;AndroidDatabase"/>
		<rdfs:seeAlso rdf:resource="&android-2_1;AndroidGraphics"/>
		<rdfs:seeAlso rdf:resource="&android-2_1;AndroidContent"/>
		<rdfs:seeAlso rdf:resource="&android-2_1;AndroidGraphicsDrawable"/>
		<rdfs:seeAlso rdf:resource="&android-2_1;AndroidMedia"/>
		<rdfs:seeAlso rdf:resource="&android-2_1;JavaUtil"/>
		<rdfs:seeAlso rdf:resource="&android-2_1;AndroidViewInputmethod"/>
		<rdfs:seeAlso rdf:resource="&android-2_1;AndroidApp"/>
		<rdfs:seeAlso rdf:resource="&android-2_1;AndroidTextMethod"/>
		<rdfs:comment xml:lang="en">Java API part implementing the android.widget package for Android 2.1</rdfs:comment>
	</owl:Class>
	<owl:Class rdf:about="&android-2_1;AndroidAppwidget">
		<rdfs:subClassOf rdf:resource="&java;JavaAPIPart"/>
		<rdfs:seeAlso rdf:resource="&android-2_1;AndroidGraphics"/>
		<rdfs:seeAlso rdf:resource="&android-2_1;AndroidContent"/>
		<rdfs:seeAlso rdf:resource="&android-2_1;AndroidWidget"/>
		<rdfs:seeAlso rdf:resource="&android-2_1;AndroidView"/>
		<rdfs:seeAlso rdf:resource="&android-2_1;JavaLang"/>
		<rdfs:seeAlso rdf:resource="&android-2_1;JavaUtil"/>
		<rdfs:seeAlso rdf:resource="&android-2_1;AndroidUtil"/>
		<rdfs:seeAlso rdf:resource="&android-2_1;AndroidOs"/>
		<rdfs:comment xml:lang="en">Java API part implementing the android.appwidget package for Android 2.1</rdfs:comment>
	</owl:Class>
	<owl:Class rdf:about="&android-2_1;AndroidBluetooth">
		<rdfs:subClassOf rdf:resource="&java;JavaAPIPart"/>
		<rdfs:seeAlso rdf:resource="&android-2_1;JavaIo"/>
		<rdfs:seeAlso rdf:resource="&android-2_1;JavaLang"/>
		<rdfs:seeAlso rdf:resource="&android-2_1;AndroidOs"/>
		<rdfs:seeAlso rdf:resource="&android-2_1;JavaUtil"/>
		<rdfs:comment xml:lang="en">Java API part implementing the android.bluetooth package for Android 2.1</rdfs:comment>
	</owl:Class>
	<owl:Class rdf:about="&android-2_1;AndroidGesture">
		<rdfs:subClassOf rdf:resource="&java;JavaAPIPart"/>
		<rdfs:seeAlso rdf:resource="&android-2_1;AndroidGraphics"/>
		<rdfs:seeAlso rdf:resource="&android-2_1;AndroidContent"/>
		<rdfs:seeAlso rdf:resource="&android-2_1;AndroidWidget"/>
		<rdfs:seeAlso rdf:resource="&android-2_1;AndroidView"/>
		<rdfs:seeAlso rdf:resource="&android-2_1;JavaLang"/>
		<rdfs:seeAlso rdf:resource="&android-2_1;JavaUtil"/>
		<rdfs:seeAlso rdf:resource="&android-2_1;JavaIo"/>
		<rdfs:seeAlso rdf:resource="&android-2_1;AndroidUtil"/>
		<rdfs:seeAlso rdf:resource="&android-2_1;AndroidOs"/>
		<rdfs:comment xml:lang="en">Java API part implementing the android.gesture package for Android 2.1</rdfs:comment>
	</owl:Class>
	<owl:Class rdf:about="&android-2_1;AndroidHardware">
		<rdfs:subClassOf rdf:resource="&android-1_6;AndroidHardware"/>
		<rdfs:seeAlso rdf:resource="&android-2_1;AndroidView"/>
		<rdfs:seeAlso rdf:resource="&android-2_1;JavaLang"/>
		<rdfs:seeAlso rdf:resource="&android-2_1;AndroidOs"/>
		<rdfs:seeAlso rdf:resource="&android-2_1;JavaUtil"/>
		<rdfs:comment xml:lang="en">Java API part implementing the android.hardware package for Android 2.1</rdfs:comment>
	</owl:Class>
	<owl:Class rdf:about="&android-2_1;AndroidInputmethodservice">
		<rdfs:subClassOf rdf:resource="&android-1_6;AndroidInputmethodservice"/>
		<rdfs:seeAlso rdf:resource="&android-2_1;AndroidGraphics"/>
		<rdfs:seeAlso rdf:resource="&android-2_1;AndroidContent"/>
		<rdfs:seeAlso rdf:resource="&android-2_1;AndroidWidget"/>
		<rdfs:seeAlso rdf:resource="&android-2_1;JavaLang"/>
		<rdfs:seeAlso rdf:resource="&android-2_1;AndroidGraphicsDrawable"/>
		<rdfs:seeAlso rdf:resource="&android-2_1;AndroidView"/>
		<rdfs:seeAlso rdf:resource="&android-2_1;JavaUtil"/>
		<rdfs:seeAlso rdf:resource="&android-2_1;AndroidViewInputmethod"/>
		<rdfs:seeAlso rdf:resource="&android-2_1;AndroidApp"/>
		<rdfs:seeAlso rdf:resource="&android-2_1;JavaIo"/>
		<rdfs:seeAlso rdf:resource="&android-2_1;AndroidContentRes"/>
		<rdfs:seeAlso rdf:resource="&android-2_1;AndroidUtil"/>
		<rdfs:seeAlso rdf:resource="&android-2_1;AndroidOs"/>
		<rdfs:comment xml:lang="en">Java API part implementing the android.inputmethodservice package for Android 2.1</rdfs:comment>
	</owl:Class>
	<owl:Class rdf:about="&android-2_1;AndroidLocation">
		<rdfs:subClassOf rdf:resource="&android-1_6;AndroidLocation"/>
		<rdfs:seeAlso rdf:resource="&android-2_1;AndroidContent"/>
		<rdfs:seeAlso rdf:resource="&android-2_1;JavaLang"/>
		<rdfs:seeAlso rdf:resource="&android-2_1;JavaUtil"/>
		<rdfs:seeAlso rdf:resource="&android-2_1;AndroidApp"/>
		<rdfs:seeAlso rdf:resource="&android-2_1;AndroidUtil"/>
		<rdfs:seeAlso rdf:resource="&android-2_1;AndroidOs"/>
		<rdfs:comment xml:lang="en">Java API part implementing the android.location package for Android 2.1</rdfs:comment>
	</owl:Class>
	<owl:Class rdf:about="&android-2_1;AndroidMedia">
		<rdfs:subClassOf rdf:resource="&android-1_6;AndroidMedia"/>
		<rdfs:seeAlso rdf:resource="&android-2_1;AndroidDatabase"/>
		<rdfs:seeAlso rdf:resource="&android-2_1;AndroidNet"/>
		<rdfs:seeAlso rdf:resource="&android-2_1;AndroidGraphics"/>
		<rdfs:seeAlso rdf:resource="&android-2_1;AndroidContent"/>
		<rdfs:seeAlso rdf:resource="&android-2_1;AndroidView"/>
		<rdfs:seeAlso rdf:resource="&android-2_1;JavaLang"/>
		<rdfs:seeAlso rdf:resource="&android-2_1;AndroidApp"/>
		<rdfs:seeAlso rdf:resource="&android-2_1;JavaIo"/>
		<rdfs:seeAlso rdf:resource="&android-2_1;AndroidContentRes"/>
		<rdfs:seeAlso rdf:resource="&android-2_1;AndroidOs"/>
		<rdfs:seeAlso rdf:resource="&android-2_1;AndroidHardware"/>
		<rdfs:seeAlso rdf:resource="&android-2_1;JavaNio"/>
		<rdfs:comment xml:lang="en">Java API part implementing the android.media package for Android 2.1</rdfs:comment>
	</owl:Class>
	<owl:Class rdf:about="&android-2_1;AndroidOpengl">
		<rdfs:subClassOf rdf:resource="&android-1_6;AndroidOpengl"/>
		<rdfs:seeAlso rdf:resource="&android-2_1;AndroidGraphics"/>
		<rdfs:seeAlso rdf:resource="&android-2_1;JavaxMicroeditionKhronosEgl"/>
		<rdfs:seeAlso rdf:resource="&android-2_1;AndroidContent"/>
		<rdfs:seeAlso rdf:resource="&android-2_1;AndroidView"/>
		<rdfs:seeAlso rdf:resource="&android-2_1;JavaLang"/>
		<rdfs:seeAlso rdf:resource="&android-2_1;JavaxMicroeditionKhronosOpengles"/>
		<rdfs:seeAlso rdf:resource="&android-2_1;JavaIo"/>
		<rdfs:seeAlso rdf:resource="&android-2_1;AndroidUtil"/>
		<rdfs:seeAlso rdf:resource="&android-2_1;JavaNio"/>
		<rdfs:comment xml:lang="en">Java API part implementing the android.opengl package for Android 2.1</rdfs:comment>
	</owl:Class>
	<owl:Class rdf:about="&android-2_1;AndroidPreference">
		<rdfs:subClassOf rdf:resource="&android-1_6;AndroidPreference"/>
		<rdfs:seeAlso rdf:resource="&android-2_1;AndroidWidget"/>
		<rdfs:seeAlso rdf:resource="&android-2_1;AndroidContent"/>
		<rdfs:seeAlso rdf:resource="&android-2_1;JavaLang"/>
		<rdfs:seeAlso rdf:resource="&android-2_1;AndroidGraphicsDrawable"/>
		<rdfs:seeAlso rdf:resource="&android-2_1;AndroidNet"/>
		<rdfs:seeAlso rdf:resource="&android-2_1;AndroidView"/>
		<rdfs:seeAlso rdf:resource="&android-2_1;AndroidApp"/>
		<rdfs:seeAlso rdf:resource="&android-2_1;AndroidContentRes"/>
		<rdfs:seeAlso rdf:resource="&android-2_1;AndroidUtil"/>
		<rdfs:seeAlso rdf:resource="&android-2_1;AndroidOs"/>
		<rdfs:comment xml:lang="en">Java API part implementing the android.preference package for Android 2.1</rdfs:comment>
	</owl:Class>
	<owl:Class rdf:about="&android-2_1;AndroidProvider">
		<rdfs:subClassOf rdf:resource="&android-1_6;AndroidProvider"/>
		<rdfs:seeAlso rdf:resource="&android-2_1;AndroidDatabase"/>
		<rdfs:seeAlso rdf:resource="&android-2_1;AndroidNet"/>
		<rdfs:seeAlso rdf:resource="&android-2_1;AndroidGraphics"/>
		<rdfs:seeAlso rdf:resource="&android-2_1;AndroidContent"/>
		<rdfs:seeAlso rdf:resource="&android-2_1;AndroidView"/>
		<rdfs:seeAlso rdf:resource="&android-2_1;JavaLang"/>
		<rdfs:seeAlso rdf:resource="&android-2_1;AndroidContentRes"/>
		<rdfs:seeAlso rdf:resource="&android-2_1;JavaIo"/>
		<rdfs:seeAlso rdf:resource="&android-2_1;AndroidUtil"/>
		<rdfs:seeAlso rdf:resource="&android-2_1;AndroidWebkit"/>
		<rdfs:seeAlso rdf:resource="&android-2_1;AndroidAccounts"/>
		<rdfs:comment xml:lang="en">Java API part implementing the android.provider package for Android 2.1</rdfs:comment>
	</owl:Class>
	<owl:Class rdf:about="&android-2_1;AndroidWebkit">
		<rdfs:subClassOf rdf:resource="&java;JavaAPIPart"/>
		<rdfs:seeAlso rdf:resource="&android-2_1;AndroidGraphics"/>
		<rdfs:seeAlso rdf:resource="&android-2_1;AndroidContent"/>
		<rdfs:seeAlso rdf:resource="&android-2_1;AndroidWidget"/>
		<rdfs:seeAlso rdf:resource="&android-2_1;AndroidNetHttp"/>
		<rdfs:seeAlso rdf:resource="&android-2_1;JavaLang"/>
		<rdfs:seeAlso rdf:resource="&android-2_1;AndroidView"/>
		<rdfs:seeAlso rdf:resource="&android-2_1;JavaUtil"/>
		<rdfs:seeAlso rdf:resource="&android-2_1;JavaIo"/>
		<rdfs:seeAlso rdf:resource="&android-2_1;AndroidUtil"/>
		<rdfs:seeAlso rdf:resource="&android-2_1;AndroidOs"/>
		<rdfs:comment xml:lang="en">Java API part implementing the android.webkit package for Android 2.1</rdfs:comment>
	</owl:Class>
	<owl:Class rdf:about="&android-2_1;AndroidSax">
		<owl:equivalentClass rdf:resource="&android-1_6;AndroidSax"/>
		<rdfs:subClassOf rdf:resource="&java;JavaAPIPart"/>
		<rdfs:seeAlso rdf:resource="&android-2_1;OrgXmlSax"/>
		<rdfs:seeAlso rdf:resource="&android-2_1;JavaLang"/>
		<rdfs:comment xml:lang="en">Java API part implementing the android.sax package for Android 2.1</rdfs:comment>
	</owl:Class>
	<owl:Class rdf:about="&android-2_1;AndroidServiceWallpaper">
		<rdfs:subClassOf rdf:resource="&java;JavaAPIPart"/>
		<rdfs:seeAlso rdf:resource="&android-2_1;AndroidApp"/>
		<rdfs:seeAlso rdf:resource="&android-2_1;AndroidContent"/>
		<rdfs:seeAlso rdf:resource="&android-2_1;AndroidView"/>
		<rdfs:seeAlso rdf:resource="&android-2_1;JavaLang"/>
		<rdfs:seeAlso rdf:resource="&android-2_1;AndroidOs"/>
		<rdfs:comment xml:lang="en">Java API part implementing the android.service.wallpaper package for Android 2.1</rdfs:comment>
	</owl:Class>
	<owl:Class rdf:about="&android-2_1;AndroidSpeech">
		<owl:equivalentClass rdf:resource="&android-1_6;AndroidSpeech"/>
		<rdfs:subClassOf rdf:resource="&java;JavaAPIPart"/>
		<rdfs:seeAlso rdf:resource="&android-2_1;JavaLang"/>
		<rdfs:comment xml:lang="en">Java API part implementing the android.speech package for Android 2.1</rdfs:comment>
	</owl:Class>
	<owl:Class rdf:about="&android-2_1;AndroidSpeechTts">
		<owl:equivalentClass rdf:resource="&android-1_6;AndroidSpeechTts"/>
		<rdfs:subClassOf rdf:resource="&java;JavaAPIPart"/>
		<rdfs:seeAlso rdf:resource="&android-2_1;AndroidContent"/>
		<rdfs:seeAlso rdf:resource="&android-2_1;JavaLang"/>
		<rdfs:seeAlso rdf:resource="&android-2_1;JavaUtil"/>
		<rdfs:comment xml:lang="en">Java API part implementing the android.speech.tts package for Android 2.1</rdfs:comment>
	</owl:Class>
	<owl:Class rdf:about="&android-2_1;AndroidTelephony">
		<rdfs:subClassOf rdf:resource="&android-1_6;AndroidTelephony"/>
		<rdfs:seeAlso rdf:resource="&android-2_1;AndroidContent"/>
		<rdfs:seeAlso rdf:resource="&android-2_1;JavaLang"/>
		<rdfs:seeAlso rdf:resource="&android-2_1;JavaUtil"/>
		<rdfs:seeAlso rdf:resource="&android-2_1;AndroidText"/>
		<rdfs:seeAlso rdf:resource="&android-2_1;AndroidApp"/>
		<rdfs:seeAlso rdf:resource="&android-2_1;AndroidOs"/>
		<rdfs:comment xml:lang="en">Java API part implementing the android.telephony package for Android 2.1</rdfs:comment>
	</owl:Class>
	<owl:Class rdf:about="&android-2_1;AndroidTelephonyCdma">
		<rdfs:subClassOf rdf:resource="&java;JavaAPIPart"/>
		<rdfs:seeAlso rdf:resource="&android-2_1;AndroidTelephony"/>
		<rdfs:seeAlso rdf:resource="&android-2_1;JavaLang"/>
		<rdfs:seeAlso rdf:resource="&android-2_1;AndroidOs"/>
		<rdfs:comment xml:lang="en">Java API part implementing the android.telephony.cdma package for Android 2.1</rdfs:comment>
	</owl:Class>
	<owl:Class rdf:about="&android-2_1;AndroidTelephonyGsm">
		<owl:equivalentClass rdf:resource="&android-1_6;AndroidTelephonyGsm"/>
		<rdfs:subClassOf rdf:resource="&java;JavaAPIPart"/>
		<rdfs:seeAlso rdf:resource="&android-2_1;AndroidTelephony"/>
		<rdfs:seeAlso rdf:resource="&android-2_1;AndroidApp"/>
		<rdfs:seeAlso rdf:resource="&android-2_1;AndroidOs"/>
		<rdfs:seeAlso rdf:resource="&android-2_1;JavaLang"/>
		<rdfs:seeAlso rdf:resource="&android-2_1;JavaUtil"/>
		<rdfs:comment xml:lang="en">Java API part implementing the android.telephony.gsm package for Android 2.1</rdfs:comment>
	</owl:Class>
	<owl:Class rdf:about="&android-2_1;AndroidText">
		<rdfs:subClassOf rdf:resource="&android-1_6;AndroidText"/>
		<rdfs:seeAlso rdf:resource="&android-2_1;JavaUtilRegex"/>
		<rdfs:seeAlso rdf:resource="&android-2_1;OrgXmlSax"/>
		<rdfs:seeAlso rdf:resource="&android-2_1;AndroidGraphics"/>
		<rdfs:seeAlso rdf:resource="&android-2_1;AndroidView"/>
		<rdfs:seeAlso rdf:resource="&android-2_1;JavaLang"/>
		<rdfs:seeAlso rdf:resource="&android-2_1;JavaUtil"/>
		<rdfs:seeAlso rdf:resource="&android-2_1;AndroidUtil"/>
		<rdfs:seeAlso rdf:resource="&android-2_1;AndroidOs"/>
		<rdfs:seeAlso rdf:resource="&android-2_1;AndroidGraphicsDrawable"/>
		<rdfs:comment xml:lang="en">Java API part implementing the android.text package for Android 2.1</rdfs:comment>
	</owl:Class>
	<owl:Class rdf:about="&android-2_1;AndroidTextFormat">
		<rdfs:subClassOf rdf:resource="&android-1_6;AndroidTextFormat"/>
		<rdfs:seeAlso rdf:resource="&android-2_1;JavaText"/>
		<rdfs:seeAlso rdf:resource="&android-2_1;AndroidContent"/>
		<rdfs:seeAlso rdf:resource="&android-2_1;JavaLang"/>
		<rdfs:seeAlso rdf:resource="&android-2_1;JavaUtil"/>
		<rdfs:comment xml:lang="en">Java API part implementing the android.text.format package for Android 2.1</rdfs:comment>
	</owl:Class>
	<owl:Class rdf:about="&android-2_1;AndroidTextMethod">
		<rdfs:subClassOf rdf:resource="&android-1_6;AndroidTextMethod"/>
		<rdfs:seeAlso rdf:resource="&android-2_1;AndroidGraphics"/>
		<rdfs:seeAlso rdf:resource="&android-2_1;AndroidContent"/>
		<rdfs:seeAlso rdf:resource="&android-2_1;AndroidWidget"/>
		<rdfs:seeAlso rdf:resource="&android-2_1;AndroidView"/>
		<rdfs:seeAlso rdf:resource="&android-2_1;JavaLang"/>
		<rdfs:seeAlso rdf:resource="&android-2_1;AndroidApp"/>
		<rdfs:seeAlso rdf:resource="&android-2_1;AndroidText"/>
		<rdfs:seeAlso rdf:resource="&android-2_1;AndroidOs"/>
		<rdfs:comment xml:lang="en">Java API part implementing the android.text.method package for Android 2.1</rdfs:comment>
	</owl:Class>
	<owl:Class rdf:about="&android-2_1;AndroidTextStyle">
		<rdfs:subClassOf rdf:resource="&android-1_6;AndroidTextStyle"/>
		<rdfs:seeAlso rdf:resource="&android-2_1;AndroidNet"/>
		<rdfs:seeAlso rdf:resource="&android-2_1;AndroidGraphics"/>
		<rdfs:seeAlso rdf:resource="&android-2_1;AndroidContent"/>
		<rdfs:seeAlso rdf:resource="&android-2_1;AndroidView"/>
		<rdfs:seeAlso rdf:resource="&android-2_1;JavaLang"/>
		<rdfs:seeAlso rdf:resource="&android-2_1;AndroidText"/>
		<rdfs:seeAlso rdf:resource="&android-2_1;AndroidContentRes"/>
		<rdfs:seeAlso rdf:resource="&android-2_1;AndroidOs"/>
		<rdfs:seeAlso rdf:resource="&android-2_1;AndroidGraphicsDrawable"/>
		<rdfs:comment xml:lang="en">Java API part implementing the android.text.style package for Android 2.1</rdfs:comment>
	</owl:Class>
	<owl:Class rdf:about="&android-2_1;AndroidTextUtil">
		<owl:equivalentClass rdf:resource="&android-1_6;AndroidTextUtil"/>
		<rdfs:subClassOf rdf:resource="&java;JavaAPIPart"/>
		<rdfs:seeAlso rdf:resource="&android-2_1;AndroidText"/>
		<rdfs:seeAlso rdf:resource="&android-2_1;JavaUtilRegex"/>
		<rdfs:seeAlso rdf:resource="&android-2_1;AndroidWidget"/>
		<rdfs:seeAlso rdf:resource="&android-2_1;JavaLang"/>
		<rdfs:comment xml:lang="en">Java API part implementing the android.text.util package for Android 2.1</rdfs:comment>
	</owl:Class>
	<owl:Class rdf:about="&android-2_1;AndroidTest">
		<rdfs:subClassOf rdf:resource="&android-1_6;AndroidTest"/>
		<rdfs:seeAlso rdf:resource="&android-2_1;JavaLangAnnotation"/>
		<rdfs:seeAlso rdf:resource="&android-2_1;AndroidTestMock"/>
		<rdfs:seeAlso rdf:resource="&android-2_1;JunitRunner"/>
		<rdfs:seeAlso rdf:resource="&android-2_1;AndroidContent"/>
		<rdfs:seeAlso rdf:resource="&android-2_1;JavaLang"/>
		<rdfs:seeAlso rdf:resource="&android-2_1;AndroidNet"/>
		<rdfs:seeAlso rdf:resource="&android-2_1;JavaUtilRegex"/>
		<rdfs:seeAlso rdf:resource="&android-2_1;JunitFramework"/>
		<rdfs:seeAlso rdf:resource="&android-2_1;AndroidView"/>
		<rdfs:seeAlso rdf:resource="&android-2_1;JavaUtil"/>
		<rdfs:seeAlso rdf:resource="&android-2_1;AndroidApp"/>
		<rdfs:seeAlso rdf:resource="&android-2_1;JavaIo"/>
		<rdfs:seeAlso rdf:resource="&android-2_1;AndroidOs"/>
		<rdfs:seeAlso rdf:resource="&android-2_1;AndroidDatabaseSqlite"/>
		<rdfs:comment xml:lang="en">Java API part implementing the android.test package for Android 2.1</rdfs:comment>
	</owl:Class>
	<owl:Class rdf:about="&android-2_1;AndroidTestMock">
		<rdfs:subClassOf rdf:resource="&android-1_6;AndroidTestMock"/>
		<rdfs:seeAlso rdf:resource="&android-2_1;AndroidContentPm"/>
		<rdfs:seeAlso rdf:resource="&android-2_1;JavaLang"/>
		<rdfs:seeAlso rdf:resource="&android-2_1;AndroidNet"/>
		<rdfs:seeAlso rdf:resource="&android-2_1;AndroidContentRes"/>
		<rdfs:seeAlso rdf:resource="&android-2_1;AndroidUtil"/>
		<rdfs:seeAlso rdf:resource="&android-2_1;AndroidOs"/>
		<rdfs:seeAlso rdf:resource="&android-2_1;AndroidDatabase"/>
		<rdfs:seeAlso rdf:resource="&android-2_1;AndroidGraphics"/>
		<rdfs:seeAlso rdf:resource="&android-2_1;AndroidContent"/>
		<rdfs:seeAlso rdf:resource="&android-2_1;AndroidGraphicsDrawable"/>
		<rdfs:seeAlso rdf:resource="&android-2_1;JavaUtil"/>
		<rdfs:seeAlso rdf:resource="&android-2_1;AndroidApp"/>
		<rdfs:seeAlso rdf:resource="&android-2_1;JavaIo"/>
		<rdfs:seeAlso rdf:resource="&android-2_1;AndroidDatabaseSqlite"/>
		<rdfs:comment xml:lang="en">Java API part implementing the android.test.mock package for Android 2.1</rdfs:comment>
	</owl:Class>
	<owl:Class rdf:about="&android-2_1;AndroidTestSuitebuilder">
		<owl:equivalentClass rdf:resource="&android-1_6;AndroidTestSuitebuilder"/>
		<rdfs:subClassOf rdf:resource="&java;JavaAPIPart"/>
		<rdfs:seeAlso rdf:resource="&android-2_1;JavaLangAnnotation"/>
		<rdfs:seeAlso rdf:resource="&android-2_1;JunitFramework"/>
		<rdfs:seeAlso rdf:resource="&android-2_1;JavaLang"/>
		<rdfs:seeAlso rdf:resource="&android-2_1;JavaUtil"/>
		<rdfs:seeAlso rdf:resource="&android-2_1;JavaLangReflect"/>
		<rdfs:comment xml:lang="en">Java API part implementing the android.test.suitebuilder package for Android 2.1</rdfs:comment>
	</owl:Class>
	<owl:Class rdf:about="&android-2_1;AndroidTestSuitebuilderAnnotation">
		<owl:equivalentClass rdf:resource="&android-1_6;AndroidTestSuitebuilderAnnotation"/>
		<rdfs:subClassOf rdf:resource="&java;JavaAPIPart"/>
		<rdfs:seeAlso rdf:resource="&android-2_1;JavaLangAnnotation"/>
		<rdfs:comment xml:lang="en">Java API part implementing the android.test.suitebuilder.annotation package for Android 2.1</rdfs:comment>
	</owl:Class>
	<owl:Class rdf:about="&android-2_1;JavaLang">
		<owl:equivalentClass rdf:resource="&android-1_6;JavaLang"/>
		<rdfs:subClassOf rdf:resource="&java;JavaAPIPart"/>
		<rdfs:seeAlso rdf:resource="&android-2_1;JavaLangAnnotation"/>
		<rdfs:seeAlso rdf:resource="&android-2_1;JavaNet"/>
		<rdfs:seeAlso rdf:resource="&android-2_1;JavaUtil"/>
		<rdfs:seeAlso rdf:resource="&android-2_1;JavaIo"/>
		<rdfs:seeAlso rdf:resource="&android-2_1;JavaNioChannels"/>
		<rdfs:seeAlso rdf:resource="&android-2_1;JavaSecurity"/>
		<rdfs:seeAlso rdf:resource="&android-2_1;JavaNio"/>
		<rdfs:seeAlso rdf:resource="&android-2_1;JavaLangReflect"/>
		<rdfs:comment xml:lang="en">Java API part implementing the java.lang package for Android 2.1</rdfs:comment>
	</owl:Class>
	<owl:Class rdf:about="&android-2_1;JavaLangAnnotation">
		<owl:equivalentClass rdf:resource="&android-1_6;JavaLangAnnotation"/>
		<rdfs:subClassOf rdf:resource="&java;JavaAPIPart"/>
		<rdfs:seeAlso rdf:resource="&android-2_1;JavaLang"/>
		<rdfs:seeAlso rdf:resource="&android-2_1;JavaLangReflect"/>
		<rdfs:comment xml:lang="en">Java API part implementing the java.lang.annotation package for Android 2.1</rdfs:comment>
	</owl:Class>
	<owl:Class rdf:about="&android-2_1;JavaLangReflect">
		<owl:equivalentClass rdf:resource="&java-se-6;JavaLangReflect"/>
		<owl:equivalentClass rdf:resource="&android-1_6;JavaLangReflect"/>
		<rdfs:subClassOf rdf:resource="&java;JavaAPIPart"/>
		<rdfs:seeAlso rdf:resource="&android-2_1;JavaLangAnnotation"/>
		<rdfs:seeAlso rdf:resource="&android-2_1;JavaIo"/>
		<rdfs:seeAlso rdf:resource="&android-2_1;JavaLang"/>
		<rdfs:seeAlso rdf:resource="&android-2_1;JavaSecurity"/>
		<rdfs:comment xml:lang="en">Java API part implementing the java.lang.reflect package for Android 2.1</rdfs:comment>
	</owl:Class>
	<owl:Class rdf:about="&android-2_1;JavaLangRef">
		<owl:equivalentClass rdf:resource="&java-se-6;JavaLangRef"/>
		<owl:equivalentClass rdf:resource="&android-1_6;JavaLangRef"/>
		<rdfs:subClassOf rdf:resource="&java;JavaAPIPart"/>
		<rdfs:seeAlso rdf:resource="&android-2_1;JavaLang"/>
		<rdfs:comment xml:lang="en">Java API part implementing the java.lang.ref package for Android 2.1</rdfs:comment>
	</owl:Class>
	<owl:Class rdf:about="&android-2_1;JavaUtil">
		<owl:equivalentClass rdf:resource="&android-1_6;JavaUtil"/>
		<rdfs:subClassOf rdf:resource="&java;JavaAPIPart"/>
		<rdfs:seeAlso rdf:resource="&android-2_1;JavaMath"/>
		<rdfs:seeAlso rdf:resource="&android-2_1;JavaLang"/>
		<rdfs:seeAlso rdf:resource="&android-2_1;JavaUtilRegex"/>
		<rdfs:seeAlso rdf:resource="&android-2_1;JavaIo"/>
		<rdfs:seeAlso rdf:resource="&android-2_1;JavaNioChannels"/>
		<rdfs:seeAlso rdf:resource="&android-2_1;JavaSecurity"/>
		<rdfs:comment xml:lang="en">Java API part implementing the java.util package for Android 2.1</rdfs:comment>
	</owl:Class>
	<owl:Class rdf:about="&android-2_1;JavaUtilConcurrent">
		<owl:equivalentClass rdf:resource="&android-1_6;JavaUtilConcurrent"/>
		<rdfs:subClassOf rdf:resource="&java;JavaAPIPart"/>
		<rdfs:seeAlso rdf:resource="&android-2_1;JavaLang"/>
		<rdfs:seeAlso rdf:resource="&android-2_1;JavaUtil"/>
		<rdfs:seeAlso rdf:resource="&android-2_1;JavaIo"/>
		<rdfs:seeAlso rdf:resource="&android-2_1;JavaSecurity"/>
		<rdfs:comment xml:lang="en">Java API part implementing the java.util.concurrent package for Android 2.1</rdfs:comment>
	</owl:Class>
	<owl:Class rdf:about="&android-2_1;JavaUtilConcurrentAtomic">
		<owl:equivalentClass rdf:resource="&android-1_6;JavaUtilConcurrentAtomic"/>
		<rdfs:subClassOf rdf:resource="&java;JavaAPIPart"/>
		<rdfs:seeAlso rdf:resource="&android-2_1;JavaIo"/>
		<rdfs:seeAlso rdf:resource="&android-2_1;JavaLang"/>
		<rdfs:comment xml:lang="en">Java API part implementing the java.util.concurrent.atomic package for Android 2.1</rdfs:comment>
	</owl:Class>
	<owl:Class rdf:about="&android-2_1;JavaUtilConcurrentLocks">
		<rdfs:subClassOf rdf:resource="&android-1_6;JavaUtilConcurrentLocks"/>
		<rdfs:seeAlso rdf:resource="&android-2_1;JavaIo"/>
		<rdfs:seeAlso rdf:resource="&android-2_1;JavaLang"/>
		<rdfs:seeAlso rdf:resource="&android-2_1;JavaUtilConcurrent"/>
		<rdfs:seeAlso rdf:resource="&android-2_1;JavaUtil"/>
		<rdfs:comment xml:lang="en">Java API part implementing the java.util.concurrent.locks package for Android 2.1</rdfs:comment>
	</owl:Class>
	<owl:Class rdf:about="&android-2_1;JavaUtilRegex">
		<owl:equivalentClass rdf:resource="&java-se-6;JavaUtilRegex"/>
		<owl:equivalentClass rdf:resource="&android-1_6;JavaUtilRegex"/>
		<rdfs:subClassOf rdf:resource="&java;JavaAPIPart"/>
		<rdfs:seeAlso rdf:resource="&android-2_1;JavaIo"/>
		<rdfs:seeAlso rdf:resource="&android-2_1;JavaLang"/>
		<rdfs:comment xml:lang="en">Java API part implementing the java.util.regex package for Android 2.1</rdfs:comment>
	</owl:Class>
	<owl:Class rdf:about="&android-2_1;JavaUtilJar">
		<owl:equivalentClass rdf:resource="&java-se-6;JavaUtilJar"/>
		<owl:equivalentClass rdf:resource="&android-1_6;JavaUtilJar"/>
		<rdfs:subClassOf rdf:resource="&java;JavaAPIPart"/>
		<rdfs:seeAlso rdf:resource="&android-2_1;JavaLang"/>
		<rdfs:seeAlso rdf:resource="&android-2_1;JavaUtil"/>
		<rdfs:seeAlso rdf:resource="&android-2_1;JavaUtilZip"/>
		<rdfs:seeAlso rdf:resource="&android-2_1;JavaBeans"/>
		<rdfs:seeAlso rdf:resource="&android-2_1;JavaIo"/>
		<rdfs:comment xml:lang="en">Java API part implementing the java.util.jar package for Android 2.1</rdfs:comment>
	</owl:Class>
	<owl:Class rdf:about="&android-2_1;JavaUtilZip">
		<owl:equivalentClass rdf:resource="&android-1_6;JavaUtilZip"/>
		<rdfs:subClassOf rdf:resource="&java;JavaAPIPart"/>
		<rdfs:seeAlso rdf:resource="&android-2_1;JavaIo"/>
		<rdfs:seeAlso rdf:resource="&android-2_1;JavaLang"/>
		<rdfs:seeAlso rdf:resource="&android-2_1;JavaUtil"/>
		<rdfs:comment xml:lang="en">Java API part implementing the java.util.zip package for Android 2.1</rdfs:comment>
	</owl:Class>
	<owl:Class rdf:about="&android-2_1;JavaUtilLogging">
		<owl:equivalentClass rdf:resource="&android-1_6;JavaUtilLogging"/>
		<rdfs:subClassOf rdf:resource="&java;JavaAPIPart"/>
		<rdfs:seeAlso rdf:resource="&android-2_1;JavaLang"/>
		<rdfs:seeAlso rdf:resource="&android-2_1;JavaUtil"/>
		<rdfs:seeAlso rdf:resource="&android-2_1;JavaBeans"/>
		<rdfs:seeAlso rdf:resource="&android-2_1;JavaIo"/>
		<rdfs:seeAlso rdf:resource="&android-2_1;JavaSecurity"/>
		<rdfs:comment xml:lang="en">Java API part implementing the java.util.logging package for Android 2.1</rdfs:comment>
	</owl:Class>
	<owl:Class rdf:about="&android-2_1;JavaUtilPrefs">
		<owl:equivalentClass rdf:resource="&java-se-6;JavaUtilPrefs"/>
		<owl:equivalentClass rdf:resource="&android-1_6;JavaUtilPrefs"/>
		<rdfs:subClassOf rdf:resource="&java;JavaAPIPart"/>
		<rdfs:seeAlso rdf:resource="&android-2_1;JavaIo"/>
		<rdfs:seeAlso rdf:resource="&android-2_1;JavaLang"/>
		<rdfs:seeAlso rdf:resource="&android-2_1;JavaUtil"/>
		<rdfs:comment xml:lang="en">Java API part implementing the java.util.prefs package for Android 2.1</rdfs:comment>
	</owl:Class>
	<owl:Class rdf:about="&android-2_1;JavaIo">
		<owl:equivalentClass rdf:resource="&android-1_6;JavaIo"/>
		<rdfs:subClassOf rdf:resource="&java;JavaAPIPart"/>
		<rdfs:seeAlso rdf:resource="&android-2_1;JavaLang"/>
		<rdfs:seeAlso rdf:resource="&android-2_1;JavaUtil"/>
		<rdfs:seeAlso rdf:resource="&android-2_1;JavaNioCharset"/>
		<rdfs:seeAlso rdf:resource="&android-2_1;JavaNioChannels"/>
		<rdfs:seeAlso rdf:resource="&android-2_1;JavaNet"/>
		<rdfs:seeAlso rdf:resource="&android-2_1;JavaNio"/>
		<rdfs:seeAlso rdf:resource="&android-2_1;JavaSecurity"/>
		<rdfs:comment xml:lang="en">Java API part implementing the java.io package for Android 2.1</rdfs:comment>
	</owl:Class>
	<owl:Class rdf:about="&android-2_1;JavaNio">
		<owl:equivalentClass rdf:resource="&android-1_6;JavaNio"/>
		<rdfs:subClassOf rdf:resource="&java;JavaAPIPart"/>
		<rdfs:seeAlso rdf:resource="&android-2_1;JavaLang"/>
		<rdfs:comment xml:lang="en">Java API part implementing the java.nio package for Android 2.1</rdfs:comment>
	</owl:Class>
	<owl:Class rdf:about="&android-2_1;JavaNioChannels">
		<owl:equivalentClass rdf:resource="&java-se-6;JavaNioChannels"/>
		<owl:equivalentClass rdf:resource="&android-1_6;JavaNioChannels"/>
		<rdfs:subClassOf rdf:resource="&java;JavaAPIPart"/>
		<rdfs:seeAlso rdf:resource="&android-2_1;JavaLang"/>
		<rdfs:seeAlso rdf:resource="&android-2_1;JavaNioChannelsSpi"/>
		<rdfs:seeAlso rdf:resource="&android-2_1;JavaUtil"/>
		<rdfs:seeAlso rdf:resource="&android-2_1;JavaIo"/>
		<rdfs:seeAlso rdf:resource="&android-2_1;JavaNioCharset"/>
		<rdfs:seeAlso rdf:resource="&android-2_1;JavaNet"/>
		<rdfs:seeAlso rdf:resource="&android-2_1;JavaNio"/>
		<rdfs:comment xml:lang="en">Java API part implementing the java.nio.channels package for Android 2.1</rdfs:comment>
	</owl:Class>
	<owl:Class rdf:about="&android-2_1;JavaNioChannelsSpi">
		<owl:equivalentClass rdf:resource="&java-se-6;JavaNioChannelsSpi"/>
		<owl:equivalentClass rdf:resource="&android-1_6;JavaNioChannelsSpi"/>
		<rdfs:subClassOf rdf:resource="&java;JavaAPIPart"/>
		<rdfs:seeAlso rdf:resource="&android-2_1;JavaLang"/>
		<rdfs:seeAlso rdf:resource="&android-2_1;JavaNioChannels"/>
		<rdfs:seeAlso rdf:resource="&android-2_1;JavaUtil"/>
		<rdfs:comment xml:lang="en">Java API part implementing the java.nio.channels.spi package for Android 2.1</rdfs:comment>
	</owl:Class>
	<owl:Class rdf:about="&android-2_1;JavaNioCharset">
		<owl:equivalentClass rdf:resource="&java-se-6;JavaNioCharset"/>
		<owl:equivalentClass rdf:resource="&android-1_6;JavaNioCharset"/>
		<rdfs:subClassOf rdf:resource="&java;JavaAPIPart"/>
		<rdfs:seeAlso rdf:resource="&android-2_1;JavaLang"/>
		<rdfs:seeAlso rdf:resource="&android-2_1;JavaUtil"/>
		<rdfs:seeAlso rdf:resource="&android-2_1;JavaIo"/>
		<rdfs:seeAlso rdf:resource="&android-2_1;JavaNio"/>
		<rdfs:comment xml:lang="en">Java API part implementing the java.nio.charset package for Android 2.1</rdfs:comment>
	</owl:Class>
	<owl:Class rdf:about="&android-2_1;JavaNioCharsetSpi">
		<owl:equivalentClass rdf:resource="&java-se-6;JavaNioCharsetSpi"/>
		<owl:equivalentClass rdf:resource="&android-1_6;JavaNioCharsetSpi"/>
		<rdfs:subClassOf rdf:resource="&java;JavaAPIPart"/>
		<rdfs:seeAlso rdf:resource="&android-2_1;JavaNioCharset"/>
		<rdfs:seeAlso rdf:resource="&android-2_1;JavaLang"/>
		<rdfs:seeAlso rdf:resource="&android-2_1;JavaUtil"/>
		<rdfs:comment xml:lang="en">Java API part implementing the java.nio.charset.spi package for Android 2.1</rdfs:comment>
	</owl:Class>
	<owl:Class rdf:about="&android-2_1;JavaNet">
		<owl:equivalentClass rdf:resource="&android-1_6;JavaNet"/>
		<rdfs:subClassOf rdf:resource="&java;JavaAPIPart"/>
		<rdfs:seeAlso rdf:resource="&android-2_1;JavaLang"/>
		<rdfs:seeAlso rdf:resource="&android-2_1;JavaUtil"/>
		<rdfs:seeAlso rdf:resource="&android-2_1;JavaIo"/>
		<rdfs:seeAlso rdf:resource="&android-2_1;JavaNioChannels"/>
		<rdfs:seeAlso rdf:resource="&android-2_1;JavaUtilJar"/>
		<rdfs:seeAlso rdf:resource="&android-2_1;JavaSecurity"/>
		<rdfs:comment xml:lang="en">Java API part implementing the java.net package for Android 2.1</rdfs:comment>
	</owl:Class>
	<owl:Class rdf:about="&android-2_1;JavaSecurity">
		<owl:equivalentClass rdf:resource="&android-1_6;JavaSecurity"/>
		<rdfs:subClassOf rdf:resource="&java;JavaAPIPart"/>
		<rdfs:seeAlso rdf:resource="&android-2_1;JavaxCrypto"/>
		<rdfs:seeAlso rdf:resource="&android-2_1;JavaSecuritySpec"/>
		<rdfs:seeAlso rdf:resource="&android-2_1;JavaLang"/>
		<rdfs:seeAlso rdf:resource="&android-2_1;JavaxSecurityAuth"/>
		<rdfs:seeAlso rdf:resource="&android-2_1;JavaxSecurityAuthCallback"/>
		<rdfs:seeAlso rdf:resource="&android-2_1;JavaNet"/>
		<rdfs:seeAlso rdf:resource="&android-2_1;JavaSecurityCert"/>
		<rdfs:seeAlso rdf:resource="&android-2_1;JavaUtil"/>
		<rdfs:seeAlso rdf:resource="&android-2_1;JavaIo"/>
		<rdfs:seeAlso rdf:resource="&android-2_1;JavaNio"/>
		<rdfs:comment xml:lang="en">Java API part implementing the java.security package for Android 2.1</rdfs:comment>
	</owl:Class>
	<owl:Class rdf:about="&android-2_1;JavaSecurityCert">
		<owl:equivalentClass rdf:resource="&java-se-6;JavaSecurityCert"/>
		<owl:equivalentClass rdf:resource="&android-1_6;JavaSecurityCert"/>
		<rdfs:subClassOf rdf:resource="&java;JavaAPIPart"/>
		<rdfs:seeAlso rdf:resource="&android-2_1;JavaMath"/>
		<rdfs:seeAlso rdf:resource="&android-2_1;JavaLang"/>
		<rdfs:seeAlso rdf:resource="&android-2_1;JavaxSecurityAuthX500"/>
		<rdfs:seeAlso rdf:resource="&android-2_1;JavaUtil"/>
		<rdfs:seeAlso rdf:resource="&android-2_1;JavaIo"/>
		<rdfs:seeAlso rdf:resource="&android-2_1;JavaSecurity"/>
		<rdfs:comment xml:lang="en">Java API part implementing the java.security.cert package for Android 2.1</rdfs:comment>
	</owl:Class>
	<owl:Class rdf:about="&android-2_1;JavaSecuritySpec">
		<owl:equivalentClass rdf:resource="&java-se-6;JavaSecuritySpec"/>
		<owl:equivalentClass rdf:resource="&android-1_6;JavaSecuritySpec"/>
		<rdfs:subClassOf rdf:resource="&java;JavaAPIPart"/>
		<rdfs:seeAlso rdf:resource="&android-2_1;JavaMath"/>
		<rdfs:seeAlso rdf:resource="&android-2_1;JavaSecurityInterfaces"/>
		<rdfs:seeAlso rdf:resource="&android-2_1;JavaLang"/>
		<rdfs:seeAlso rdf:resource="&android-2_1;JavaSecurity"/>
		<rdfs:comment xml:lang="en">Java API part implementing the java.security.spec package for Android 2.1</rdfs:comment>
	</owl:Class>
	<owl:Class rdf:about="&android-2_1;JavaSecurityAcl">
		<owl:equivalentClass rdf:resource="&java-se-6;JavaSecurityAcl"/>
		<owl:equivalentClass rdf:resource="&android-1_6;JavaSecurityAcl"/>
		<rdfs:subClassOf rdf:resource="&java;JavaAPIPart"/>
		<rdfs:seeAlso rdf:resource="&android-2_1;JavaLang"/>
		<rdfs:seeAlso rdf:resource="&android-2_1;JavaUtil"/>
		<rdfs:seeAlso rdf:resource="&android-2_1;JavaSecurity"/>
		<rdfs:comment xml:lang="en">Java API part implementing the java.security.acl package for Android 2.1</rdfs:comment>
	</owl:Class>
	<owl:Class rdf:about="&android-2_1;JavaSecurityInterfaces">
		<owl:equivalentClass rdf:resource="&java-se-6;JavaSecurityInterfaces"/>
		<owl:equivalentClass rdf:resource="&android-1_6;JavaSecurityInterfaces"/>
		<rdfs:subClassOf rdf:resource="&java;JavaAPIPart"/>
		<rdfs:seeAlso rdf:resource="&android-2_1;JavaMath"/>
		<rdfs:seeAlso rdf:resource="&android-2_1;JavaSecuritySpec"/>
		<rdfs:seeAlso rdf:resource="&android-2_1;JavaSecurity"/>
		<rdfs:comment xml:lang="en">Java API part implementing the java.security.interfaces package for Android 2.1</rdfs:comment>
	</owl:Class>
	<owl:Class rdf:about="&android-2_1;JavaText">
		<owl:equivalentClass rdf:resource="&android-1_6;JavaText"/>
		<rdfs:subClassOf rdf:resource="&java;JavaAPIPart"/>
		<rdfs:seeAlso rdf:resource="&android-2_1;JavaLang"/>
		<rdfs:seeAlso rdf:resource="&android-2_1;JavaUtil"/>
		<rdfs:seeAlso rdf:resource="&android-2_1;JavaIo"/>
		<rdfs:comment xml:lang="en">Java API part implementing the java.text package for Android 2.1</rdfs:comment>
	</owl:Class>
	<owl:Class rdf:about="&android-2_1;JavaAwtFont">
		<owl:equivalentClass rdf:resource="&android-1_6;JavaAwtFont"/>
		<rdfs:subClassOf rdf:resource="&java;JavaAPIPart"/>
		<rdfs:seeAlso rdf:resource="&android-2_1;JavaText"/>
		<rdfs:seeAlso rdf:resource="&android-2_1;JavaIo"/>
		<rdfs:seeAlso rdf:resource="&android-2_1;JavaLang"/>
		<rdfs:comment xml:lang="en">Java API part implementing the java.awt.font package for Android 2.1</rdfs:comment>
	</owl:Class>
	<owl:Class rdf:about="&android-2_1;JavaBeans">
		<owl:equivalentClass rdf:resource="&android-1_6;JavaBeans"/>
		<rdfs:subClassOf rdf:resource="&java;JavaAPIPart"/>
		<rdfs:seeAlso rdf:resource="&android-2_1;JavaIo"/>
		<rdfs:seeAlso rdf:resource="&android-2_1;JavaLang"/>
		<rdfs:seeAlso rdf:resource="&android-2_1;JavaUtil"/>
		<rdfs:comment xml:lang="en">Java API part implementing the java.beans package for Android 2.1</rdfs:comment>
	</owl:Class>
	<owl:Class rdf:about="&android-2_1;JavaMath">
		<owl:equivalentClass rdf:resource="&android-1_6;JavaMath"/>
		<rdfs:subClassOf rdf:resource="&java;JavaAPIPart"/>
		<rdfs:seeAlso rdf:resource="&android-2_1;JavaIo"/>
		<rdfs:seeAlso rdf:resource="&android-2_1;JavaLang"/>
		<rdfs:seeAlso rdf:resource="&android-2_1;JavaUtil"/>
		<rdfs:comment xml:lang="en">Java API part implementing the java.math package for Android 2.1</rdfs:comment>
	</owl:Class>
	<owl:Class rdf:about="&android-2_1;JavaSql">
		<owl:equivalentClass rdf:resource="&android-1_6;JavaSql"/>
		<rdfs:subClassOf rdf:resource="&java;JavaAPIPart"/>
		<rdfs:seeAlso rdf:resource="&android-2_1;JavaMath"/>
		<rdfs:seeAlso rdf:resource="&android-2_1;JavaLang"/>
		<rdfs:seeAlso rdf:resource="&android-2_1;JavaUtil"/>
		<rdfs:seeAlso rdf:resource="&android-2_1;JavaIo"/>
		<rdfs:seeAlso rdf:resource="&android-2_1;JavaNet"/>
		<rdfs:seeAlso rdf:resource="&android-2_1;JavaSecurity"/>
		<rdfs:comment xml:lang="en">Java API part implementing the java.sql package for Android 2.1</rdfs:comment>
	</owl:Class>
	<owl:Class rdf:about="&android-2_1;OrgXmlpullV1">
		<owl:equivalentClass rdf:resource="&android-1_6;OrgXmlpullV1"/>
		<rdfs:subClassOf rdf:resource="&java;JavaAPIPart"/>
		<rdfs:seeAlso rdf:resource="&android-2_1;JavaLang"/>
		<rdfs:seeAlso rdf:resource="&android-2_1;JavaUtil"/>
		<rdfs:seeAlso rdf:resource="&android-2_1;JavaIo"/>
		<rdfs:comment xml:lang="en">Java API part implementing the org.xmlpull.v1 package for Android 2.1</rdfs:comment>
	</owl:Class>
	<owl:Class rdf:about="&android-2_1;OrgXmlpullV1Sax2">
		<owl:equivalentClass rdf:resource="&android-1_6;OrgXmlpullV1Sax2"/>
		<rdfs:subClassOf rdf:resource="&java;JavaAPIPart"/>
		<rdfs:seeAlso rdf:resource="&android-2_1;OrgXmlSax"/>
		<rdfs:seeAlso rdf:resource="&android-2_1;JavaLang"/>
		<rdfs:seeAlso rdf:resource="&android-2_1;OrgXmlpullV1"/>
		<rdfs:comment xml:lang="en">Java API part implementing the org.xmlpull.v1.sax2 package for Android 2.1</rdfs:comment>
	</owl:Class>
	<owl:Class rdf:about="&android-2_1;OrgXmlSax">
		<owl:equivalentClass rdf:resource="&java-se-6;OrgXmlSax"/>
		<owl:equivalentClass rdf:resource="&android-1_6;OrgXmlSax"/>
		<rdfs:subClassOf rdf:resource="&java;JavaAPIPart"/>
		<rdfs:seeAlso rdf:resource="&android-2_1;JavaIo"/>
		<rdfs:seeAlso rdf:resource="&android-2_1;JavaLang"/>
		<rdfs:seeAlso rdf:resource="&android-2_1;JavaUtil"/>
		<rdfs:comment xml:lang="en">Java API part implementing the org.xml.sax package for Android 2.1</rdfs:comment>
	</owl:Class>
	<owl:Class rdf:about="&android-2_1;OrgXmlSaxHelpers">
		<owl:equivalentClass rdf:resource="&java-se-6;OrgXmlSaxHelpers"/>
		<owl:equivalentClass rdf:resource="&android-1_6;OrgXmlSaxHelpers"/>
		<rdfs:subClassOf rdf:resource="&java;JavaAPIPart"/>
		<rdfs:seeAlso rdf:resource="&android-2_1;OrgXmlSax"/>
		<rdfs:seeAlso rdf:resource="&android-2_1;JavaLang"/>
		<rdfs:seeAlso rdf:resource="&android-2_1;JavaUtil"/>
		<rdfs:comment xml:lang="en">Java API part implementing the org.xml.sax.helpers package for Android 2.1</rdfs:comment>
	</owl:Class>
	<owl:Class rdf:about="&android-2_1;OrgXmlSaxExt">
		<owl:equivalentClass rdf:resource="&java-se-6;OrgXmlSaxExt"/>
		<owl:equivalentClass rdf:resource="&android-1_6;OrgXmlSaxExt"/>
		<rdfs:subClassOf rdf:resource="&java;JavaAPIPart"/>
		<rdfs:seeAlso rdf:resource="&android-2_1;OrgXmlSaxHelpers"/>
		<rdfs:seeAlso rdf:resource="&android-2_1;OrgXmlSax"/>
		<rdfs:seeAlso rdf:resource="&android-2_1;JavaLang"/>
		<rdfs:comment xml:lang="en">Java API part implementing the org.xml.sax.ext package for Android 2.1</rdfs:comment>
	</owl:Class>
	<owl:Class rdf:about="&android-2_1;OrgW3cDom">
		<owl:equivalentClass rdf:resource="&android-1_6;OrgW3cDom"/>
		<rdfs:subClassOf rdf:resource="&java;JavaAPIPart"/>
		<rdfs:seeAlso rdf:resource="&android-2_1;JavaLang"/>
		<rdfs:comment xml:lang="en">Java API part implementing the org.w3c.dom package for Android 2.1</rdfs:comment>
	</owl:Class>
	<owl:Class rdf:about="&android-2_1;OrgApacheCommonsLogging">
		<owl:equivalentClass rdf:resource="&android-1_6;OrgApacheCommonsLogging"/>
		<rdfs:subClassOf rdf:resource="&java;JavaAPIPart"/>
		<rdfs:seeAlso rdf:resource="&android-2_1;JavaLang"/>
		<rdfs:comment xml:lang="en">Java API part implementing the org.apache.commons.logging package for Android 2.1</rdfs:comment>
	</owl:Class>
	<owl:Class rdf:about="&android-2_1;OrgApacheHttp">
		<owl:equivalentClass rdf:resource="&android-1_6;OrgApacheHttp"/>
		<rdfs:subClassOf rdf:resource="&java;JavaAPIPart"/>
		<rdfs:seeAlso rdf:resource="&android-2_1;JavaLang"/>
		<rdfs:seeAlso rdf:resource="&android-2_1;OrgApacheHttpUtil"/>
		<rdfs:seeAlso rdf:resource="&android-2_1;JavaUtil"/>
		<rdfs:seeAlso rdf:resource="&android-2_1;OrgApacheHttpProtocol"/>
		<rdfs:seeAlso rdf:resource="&android-2_1;OrgApacheHttpParams"/>
		<rdfs:seeAlso rdf:resource="&android-2_1;JavaIo"/>
		<rdfs:seeAlso rdf:resource="&android-2_1;JavaNet"/>
		<rdfs:comment xml:lang="en">Java API part implementing the org.apache.http package for Android 2.1</rdfs:comment>
	</owl:Class>
	<owl:Class rdf:about="&android-2_1;OrgApacheHttpProtocol">
		<owl:equivalentClass rdf:resource="&android-1_6;OrgApacheHttpProtocol"/>
		<rdfs:subClassOf rdf:resource="&java;JavaAPIPart"/>
		<rdfs:seeAlso rdf:resource="&android-2_1;JavaLang"/>
		<rdfs:seeAlso rdf:resource="&android-2_1;JavaUtil"/>
		<rdfs:seeAlso rdf:resource="&android-2_1;OrgApacheHttpParams"/>
		<rdfs:seeAlso rdf:resource="&android-2_1;OrgApacheHttp"/>
		<rdfs:comment xml:lang="en">Java API part implementing the org.apache.http.protocol package for Android 2.1</rdfs:comment>
	</owl:Class>
	<owl:Class rdf:about="&android-2_1;OrgApacheHttpUtil">
		<owl:equivalentClass rdf:resource="&android-1_6;OrgApacheHttpUtil"/>
		<rdfs:subClassOf rdf:resource="&java;JavaAPIPart"/>
		<rdfs:seeAlso rdf:resource="&android-2_1;OrgApacheHttp"/>
		<rdfs:seeAlso rdf:resource="&android-2_1;JavaLang"/>
		<rdfs:seeAlso rdf:resource="&android-2_1;JavaUtil"/>
		<rdfs:comment xml:lang="en">Java API part implementing the org.apache.http.util package for Android 2.1</rdfs:comment>
	</owl:Class>
	<owl:Class rdf:about="&android-2_1;OrgApacheHttpParams">
		<owl:equivalentClass rdf:resource="&android-1_6;OrgApacheHttpParams"/>
		<rdfs:subClassOf rdf:resource="&java;JavaAPIPart"/>
		<rdfs:seeAlso rdf:resource="&android-2_1;JavaIo"/>
		<rdfs:seeAlso rdf:resource="&android-2_1;OrgApacheHttp"/>
		<rdfs:seeAlso rdf:resource="&android-2_1;JavaLang"/>
		<rdfs:comment xml:lang="en">Java API part implementing the org.apache.http.params package for Android 2.1</rdfs:comment>
	</owl:Class>
	<owl:Class rdf:about="&android-2_1;OrgApacheHttpAuth">
		<owl:equivalentClass rdf:resource="&android-1_6;OrgApacheHttpAuth"/>
		<rdfs:subClassOf rdf:resource="&java;JavaAPIPart"/>
		<rdfs:seeAlso rdf:resource="&android-2_1;OrgApacheHttpParams"/>
		<rdfs:seeAlso rdf:resource="&android-2_1;OrgApacheHttp"/>
		<rdfs:seeAlso rdf:resource="&android-2_1;JavaLang"/>
		<rdfs:seeAlso rdf:resource="&android-2_1;JavaUtil"/>
		<rdfs:seeAlso rdf:resource="&android-2_1;JavaSecurity"/>
		<rdfs:comment xml:lang="en">Java API part implementing the org.apache.http.auth package for Android 2.1</rdfs:comment>
	</owl:Class>
	<owl:Class rdf:about="&android-2_1;OrgApacheHttpAuthParams">
		<owl:equivalentClass rdf:resource="&android-1_6;OrgApacheHttpAuthParams"/>
		<rdfs:subClassOf rdf:resource="&java;JavaAPIPart"/>
		<rdfs:seeAlso rdf:resource="&android-2_1;OrgApacheHttpParams"/>
		<rdfs:seeAlso rdf:resource="&android-2_1;JavaLang"/>
		<rdfs:comment xml:lang="en">Java API part implementing the org.apache.http.auth.params package for Android 2.1</rdfs:comment>
	</owl:Class>
	<owl:Class rdf:about="&android-2_1;OrgApacheHttpClient">
		<owl:equivalentClass rdf:resource="&android-1_6;OrgApacheHttpClient"/>
		<rdfs:subClassOf rdf:resource="&java;JavaAPIPart"/>
		<rdfs:seeAlso rdf:resource="&android-2_1;OrgApacheHttpClientMethods"/>
		<rdfs:seeAlso rdf:resource="&android-2_1;JavaLang"/>
		<rdfs:seeAlso rdf:resource="&android-2_1;JavaUtil"/>
		<rdfs:seeAlso rdf:resource="&android-2_1;OrgApacheHttpProtocol"/>
		<rdfs:seeAlso rdf:resource="&android-2_1;OrgApacheHttpParams"/>
		<rdfs:seeAlso rdf:resource="&android-2_1;OrgApacheHttpAuth"/>
		<rdfs:seeAlso rdf:resource="&android-2_1;JavaIo"/>
		<rdfs:seeAlso rdf:resource="&android-2_1;OrgApacheHttpCookie"/>
		<rdfs:seeAlso rdf:resource="&android-2_1;OrgApacheHttp"/>
		<rdfs:seeAlso rdf:resource="&android-2_1;JavaNet"/>
		<rdfs:seeAlso rdf:resource="&android-2_1;OrgApacheHttpConn"/>
		<rdfs:comment xml:lang="en">Java API part implementing the org.apache.http.client package for Android 2.1</rdfs:comment>
	</owl:Class>
	<owl:Class rdf:about="&android-2_1;OrgApacheHttpClientMethods">
		<owl:equivalentClass rdf:resource="&android-1_6;OrgApacheHttpClientMethods"/>
		<rdfs:subClassOf rdf:resource="&java;JavaAPIPart"/>
		<rdfs:seeAlso rdf:resource="&android-2_1;OrgApacheHttpMessage"/>
		<rdfs:seeAlso rdf:resource="&android-2_1;JavaLang"/>
		<rdfs:seeAlso rdf:resource="&android-2_1;JavaUtil"/>
		<rdfs:seeAlso rdf:resource="&android-2_1;OrgApacheHttp"/>
		<rdfs:seeAlso rdf:resource="&android-2_1;JavaNet"/>
		<rdfs:seeAlso rdf:resource="&android-2_1;OrgApacheHttpConn"/>
		<rdfs:comment xml:lang="en">Java API part implementing the org.apache.http.client.methods package for Android 2.1</rdfs:comment>
	</owl:Class>
	<owl:Class rdf:about="&android-2_1;OrgApacheHttpClientEntity">
		<owl:equivalentClass rdf:resource="&android-1_6;OrgApacheHttpClientEntity"/>
		<rdfs:subClassOf rdf:resource="&java;JavaAPIPart"/>
		<rdfs:seeAlso rdf:resource="&android-2_1;OrgApacheHttpEntity"/>
		<rdfs:seeAlso rdf:resource="&android-2_1;JavaLang"/>
		<rdfs:seeAlso rdf:resource="&android-2_1;JavaUtil"/>
		<rdfs:comment xml:lang="en">Java API part implementing the org.apache.http.client.entity package for Android 2.1</rdfs:comment>
	</owl:Class>
	<owl:Class rdf:about="&android-2_1;OrgApacheHttpClientParams">
		<owl:equivalentClass rdf:resource="&android-1_6;OrgApacheHttpClientParams"/>
		<rdfs:subClassOf rdf:resource="&java;JavaAPIPart"/>
		<rdfs:seeAlso rdf:resource="&android-2_1;JavaLang"/>
		<rdfs:seeAlso rdf:resource="&android-2_1;JavaUtil"/>
		<rdfs:seeAlso rdf:resource="&android-2_1;OrgApacheHttpParams"/>
		<rdfs:seeAlso rdf:resource="&android-2_1;OrgApacheHttpConnParams"/>
		<rdfs:seeAlso rdf:resource="&android-2_1;OrgApacheHttpAuthParams"/>
		<rdfs:seeAlso rdf:resource="&android-2_1;OrgApacheHttp"/>
		<rdfs:seeAlso rdf:resource="&android-2_1;OrgApacheHttpCookieParams"/>
		<rdfs:seeAlso rdf:resource="&android-2_1;OrgApacheHttpConn"/>
		<rdfs:comment xml:lang="en">Java API part implementing the org.apache.http.client.params package for Android 2.1</rdfs:comment>
	</owl:Class>
	<owl:Class rdf:about="&android-2_1;OrgApacheHttpClientProtocol">
		<owl:equivalentClass rdf:resource="&android-1_6;OrgApacheHttpClientProtocol"/>
		<rdfs:subClassOf rdf:resource="&java;JavaAPIPart"/>
		<rdfs:seeAlso rdf:resource="&android-2_1;JavaLang"/>
		<rdfs:seeAlso rdf:resource="&android-2_1;JavaUtil"/>
		<rdfs:seeAlso rdf:resource="&android-2_1;OrgApacheHttpProtocol"/>
		<rdfs:seeAlso rdf:resource="&android-2_1;OrgApacheHttpAuth"/>
		<rdfs:seeAlso rdf:resource="&android-2_1;OrgApacheHttpCookie"/>
		<rdfs:seeAlso rdf:resource="&android-2_1;OrgApacheHttp"/>
		<rdfs:seeAlso rdf:resource="&android-2_1;OrgApacheHttpClient"/>
		<rdfs:comment xml:lang="en">Java API part implementing the org.apache.http.client.protocol package for Android 2.1</rdfs:comment>
	</owl:Class>
	<owl:Class rdf:about="&android-2_1;OrgApacheHttpClientUtils">
		<owl:equivalentClass rdf:resource="&android-1_6;OrgApacheHttpClientUtils"/>
		<rdfs:subClassOf rdf:resource="&java;JavaAPIPart"/>
		<rdfs:seeAlso rdf:resource="&android-2_1;OrgApacheHttp"/>
		<rdfs:seeAlso rdf:resource="&android-2_1;JavaLang"/>
		<rdfs:seeAlso rdf:resource="&android-2_1;JavaNet"/>
		<rdfs:seeAlso rdf:resource="&android-2_1;JavaUtil"/>
		<rdfs:comment xml:lang="en">Java API part implementing the org.apache.http.client.utils package for Android 2.1</rdfs:comment>
	</owl:Class>
	<owl:Class rdf:about="&android-2_1;OrgApacheHttpCookie">
		<owl:equivalentClass rdf:resource="&android-1_6;OrgApacheHttpCookie"/>
		<rdfs:subClassOf rdf:resource="&java;JavaAPIPart"/>
		<rdfs:seeAlso rdf:resource="&android-2_1;OrgApacheHttpParams"/>
		<rdfs:seeAlso rdf:resource="&android-2_1;JavaIo"/>
		<rdfs:seeAlso rdf:resource="&android-2_1;OrgApacheHttp"/>
		<rdfs:seeAlso rdf:resource="&android-2_1;JavaLang"/>
		<rdfs:seeAlso rdf:resource="&android-2_1;JavaUtil"/>
		<rdfs:comment xml:lang="en">Java API part implementing the org.apache.http.cookie package for Android 2.1</rdfs:comment>
	</owl:Class>
	<owl:Class rdf:about="&android-2_1;OrgApacheHttpCookieParams">
		<owl:equivalentClass rdf:resource="&android-1_6;OrgApacheHttpCookieParams"/>
		<rdfs:subClassOf rdf:resource="&java;JavaAPIPart"/>
		<rdfs:seeAlso rdf:resource="&android-2_1;OrgApacheHttpParams"/>
		<rdfs:seeAlso rdf:resource="&android-2_1;JavaLang"/>
		<rdfs:seeAlso rdf:resource="&android-2_1;JavaUtil"/>
		<rdfs:comment xml:lang="en">Java API part implementing the org.apache.http.cookie.params package for Android 2.1</rdfs:comment>
	</owl:Class>
	<owl:Class rdf:about="&android-2_1;OrgApacheHttpConn">
		<owl:equivalentClass rdf:resource="&android-1_6;OrgApacheHttpConn"/>
		<rdfs:subClassOf rdf:resource="&java;JavaAPIPart"/>
		<rdfs:seeAlso rdf:resource="&android-2_1;JavaLang"/>
		<rdfs:seeAlso rdf:resource="&android-2_1;OrgApacheHttpConnScheme"/>
		<rdfs:seeAlso rdf:resource="&android-2_1;OrgApacheHttpProtocol"/>
		<rdfs:seeAlso rdf:resource="&android-2_1;OrgApacheHttpParams"/>
		<rdfs:seeAlso rdf:resource="&android-2_1;OrgApacheHttpConnRouting"/>
		<rdfs:seeAlso rdf:resource="&android-2_1;JavaIo"/>
		<rdfs:seeAlso rdf:resource="&android-2_1;JavaxNetSsl"/>
		<rdfs:seeAlso rdf:resource="&android-2_1;OrgApacheHttpEntity"/>
		<rdfs:seeAlso rdf:resource="&android-2_1;OrgApacheHttp"/>
		<rdfs:seeAlso rdf:resource="&android-2_1;JavaNet"/>
		<rdfs:seeAlso rdf:resource="&android-2_1;JavaUtilConcurrent"/>
		<rdfs:comment xml:lang="en">Java API part implementing the org.apache.http.conn package for Android 2.1</rdfs:comment>
	</owl:Class>
	<owl:Class rdf:about="&android-2_1;OrgApacheHttpConnParams">
		<owl:equivalentClass rdf:resource="&android-1_6;OrgApacheHttpConnParams"/>
		<rdfs:subClassOf rdf:resource="&java;JavaAPIPart"/>
		<rdfs:seeAlso rdf:resource="&android-2_1;OrgApacheHttpParams"/>
		<rdfs:seeAlso rdf:resource="&android-2_1;OrgApacheHttpConnRouting"/>
		<rdfs:seeAlso rdf:resource="&android-2_1;OrgApacheHttp"/>
		<rdfs:seeAlso rdf:resource="&android-2_1;JavaLang"/>
		<rdfs:seeAlso rdf:resource="&android-2_1;JavaNet"/>
		<rdfs:seeAlso rdf:resource="&android-2_1;JavaUtil"/>
		<rdfs:comment xml:lang="en">Java API part implementing the org.apache.http.conn.params package for Android 2.1</rdfs:comment>
	</owl:Class>
	<owl:Class rdf:about="&android-2_1;OrgApacheHttpConnScheme">
		<owl:equivalentClass rdf:resource="&android-1_6;OrgApacheHttpConnScheme"/>
		<rdfs:subClassOf rdf:resource="&java;JavaAPIPart"/>
		<rdfs:seeAlso rdf:resource="&android-2_1;OrgApacheHttpParams"/>
		<rdfs:seeAlso rdf:resource="&android-2_1;OrgApacheHttp"/>
		<rdfs:seeAlso rdf:resource="&android-2_1;JavaLang"/>
		<rdfs:seeAlso rdf:resource="&android-2_1;JavaNet"/>
		<rdfs:seeAlso rdf:resource="&android-2_1;JavaUtil"/>
		<rdfs:comment xml:lang="en">Java API part implementing the org.apache.http.conn.scheme package for Android 2.1</rdfs:comment>
	</owl:Class>
	<owl:Class rdf:about="&android-2_1;OrgApacheHttpConnRouting">
		<owl:equivalentClass rdf:resource="&android-1_6;OrgApacheHttpConnRouting"/>
		<rdfs:subClassOf rdf:resource="&java;JavaAPIPart"/>
		<rdfs:seeAlso rdf:resource="&android-2_1;OrgApacheHttpProtocol"/>
		<rdfs:seeAlso rdf:resource="&android-2_1;OrgApacheHttp"/>
		<rdfs:seeAlso rdf:resource="&android-2_1;JavaLang"/>
		<rdfs:seeAlso rdf:resource="&android-2_1;JavaNet"/>
		<rdfs:comment xml:lang="en">Java API part implementing the org.apache.http.conn.routing package for Android 2.1</rdfs:comment>
	</owl:Class>
	<owl:Class rdf:about="&android-2_1;OrgApacheHttpConnSsl">
		<owl:equivalentClass rdf:resource="&android-1_6;OrgApacheHttpConnSsl"/>
		<rdfs:subClassOf rdf:resource="&java;JavaAPIPart"/>
		<rdfs:seeAlso rdf:resource="&android-2_1;JavaSecurityCert"/>
		<rdfs:seeAlso rdf:resource="&android-2_1;JavaLang"/>
		<rdfs:seeAlso rdf:resource="&android-2_1;OrgApacheHttpConnScheme"/>
		<rdfs:seeAlso rdf:resource="&android-2_1;OrgApacheHttpParams"/>
		<rdfs:seeAlso rdf:resource="&android-2_1;JavaxNetSsl"/>
		<rdfs:seeAlso rdf:resource="&android-2_1;JavaNet"/>
		<rdfs:seeAlso rdf:resource="&android-2_1;JavaSecurity"/>
		<rdfs:comment xml:lang="en">Java API part implementing the org.apache.http.conn.ssl package for Android 2.1</rdfs:comment>
	</owl:Class>
	<owl:Class rdf:about="&android-2_1;OrgApacheHttpConnUtil">
		<owl:equivalentClass rdf:resource="&android-1_6;OrgApacheHttpConnUtil"/>
		<rdfs:subClassOf rdf:resource="&java;JavaAPIPart"/>
		<rdfs:seeAlso rdf:resource="&android-2_1;JavaLang"/>
		<rdfs:comment xml:lang="en">Java API part implementing the org.apache.http.conn.util package for Android 2.1</rdfs:comment>
	</owl:Class>
	<owl:Class rdf:about="&android-2_1;OrgApacheHttpEntity">
		<owl:equivalentClass rdf:resource="&android-1_6;OrgApacheHttpEntity"/>
		<rdfs:subClassOf rdf:resource="&java;JavaAPIPart"/>
		<rdfs:seeAlso rdf:resource="&android-2_1;JavaIo"/>
		<rdfs:seeAlso rdf:resource="&android-2_1;OrgApacheHttp"/>
		<rdfs:seeAlso rdf:resource="&android-2_1;JavaLang"/>
		<rdfs:comment xml:lang="en">Java API part implementing the org.apache.http.entity package for Android 2.1</rdfs:comment>
	</owl:Class>
	<owl:Class rdf:about="&android-2_1;OrgApacheHttpMessage">
		<owl:equivalentClass rdf:resource="&android-1_6;OrgApacheHttpMessage"/>
		<rdfs:subClassOf rdf:resource="&java;JavaAPIPart"/>
		<rdfs:seeAlso rdf:resource="&android-2_1;JavaLang"/>
		<rdfs:seeAlso rdf:resource="&android-2_1;OrgApacheHttpUtil"/>
		<rdfs:seeAlso rdf:resource="&android-2_1;JavaUtil"/>
		<rdfs:seeAlso rdf:resource="&android-2_1;OrgApacheHttpParams"/>
		<rdfs:seeAlso rdf:resource="&android-2_1;OrgApacheHttp"/>
		<rdfs:comment xml:lang="en">Java API part implementing the org.apache.http.message package for Android 2.1</rdfs:comment>
	</owl:Class>
	<owl:Class rdf:about="&android-2_1;OrgApacheHttpImpl">
		<owl:equivalentClass rdf:resource="&android-1_6;OrgApacheHttpImpl"/>
		<rdfs:subClassOf rdf:resource="&java;JavaAPIPart"/>
		<rdfs:seeAlso rdf:resource="&android-2_1;JavaLang"/>
		<rdfs:seeAlso rdf:resource="&android-2_1;OrgApacheHttpParams"/>
		<rdfs:seeAlso rdf:resource="&android-2_1;OrgApacheHttp"/>
		<rdfs:seeAlso rdf:resource="&android-2_1;JavaNet"/>
		<rdfs:seeAlso rdf:resource="&android-2_1;OrgApacheHttpImplEntity"/>
		<rdfs:seeAlso rdf:resource="&android-2_1;JavaUtil"/>
		<rdfs:seeAlso rdf:resource="&android-2_1;OrgApacheHttpIo"/>
		<rdfs:seeAlso rdf:resource="&android-2_1;OrgApacheHttpProtocol"/>
		<rdfs:comment xml:lang="en">Java API part implementing the org.apache.http.impl package for Android 2.1</rdfs:comment>
	</owl:Class>
	<owl:Class rdf:about="&android-2_1;OrgApacheHttpImplEntity">
		<owl:equivalentClass rdf:resource="&android-1_6;OrgApacheHttpImplEntity"/>
		<rdfs:subClassOf rdf:resource="&java;JavaAPIPart"/>
		<rdfs:seeAlso rdf:resource="&android-2_1;OrgApacheHttpIo"/>
		<rdfs:seeAlso rdf:resource="&android-2_1;JavaIo"/>
		<rdfs:seeAlso rdf:resource="&android-2_1;OrgApacheHttpEntity"/>
		<rdfs:seeAlso rdf:resource="&android-2_1;OrgApacheHttp"/>
		<rdfs:seeAlso rdf:resource="&android-2_1;JavaLang"/>
		<rdfs:comment xml:lang="en">Java API part implementing the org.apache.http.impl.entity package for Android 2.1</rdfs:comment>
	</owl:Class>
	<owl:Class rdf:about="&android-2_1;OrgApacheHttpImplAuth">
		<owl:equivalentClass rdf:resource="&android-1_6;OrgApacheHttpImplAuth"/>
		<rdfs:subClassOf rdf:resource="&java;JavaAPIPart"/>
		<rdfs:seeAlso rdf:resource="&android-2_1;JavaLang"/>
		<rdfs:seeAlso rdf:resource="&android-2_1;OrgApacheHttpUtil"/>
		<rdfs:seeAlso rdf:resource="&android-2_1;JavaUtil"/>
		<rdfs:seeAlso rdf:resource="&android-2_1;OrgApacheHttpParams"/>
		<rdfs:seeAlso rdf:resource="&android-2_1;OrgApacheHttpAuth"/>
		<rdfs:seeAlso rdf:resource="&android-2_1;OrgApacheHttp"/>
		<rdfs:comment xml:lang="en">Java API part implementing the org.apache.http.impl.auth package for Android 2.1</rdfs:comment>
	</owl:Class>
	<owl:Class rdf:about="&android-2_1;OrgApacheHttpImplClient">
		<owl:equivalentClass rdf:resource="&android-1_6;OrgApacheHttpImplClient"/>
		<rdfs:subClassOf rdf:resource="&java;JavaAPIPart"/>
		<rdfs:seeAlso rdf:resource="&android-2_1;JavaLang"/>
		<rdfs:seeAlso rdf:resource="&android-2_1;OrgApacheHttpParams"/>
		<rdfs:seeAlso rdf:resource="&android-2_1;OrgApacheHttpConnRouting"/>
		<rdfs:seeAlso rdf:resource="&android-2_1;OrgApacheHttpCookie"/>
		<rdfs:seeAlso rdf:resource="&android-2_1;OrgApacheHttp"/>
		<rdfs:seeAlso rdf:resource="&android-2_1;OrgApacheHttpClient"/>
		<rdfs:seeAlso rdf:resource="&android-2_1;JavaNet"/>
		<rdfs:seeAlso rdf:resource="&android-2_1;OrgApacheHttpMessage"/>
		<rdfs:seeAlso rdf:resource="&android-2_1;OrgApacheHttpClientMethods"/>
		<rdfs:seeAlso rdf:resource="&android-2_1;JavaUtil"/>
		<rdfs:seeAlso rdf:resource="&android-2_1;OrgApacheHttpAuth"/>
		<rdfs:seeAlso rdf:resource="&android-2_1;OrgApacheHttpProtocol"/>
		<rdfs:seeAlso rdf:resource="&android-2_1;JavaIo"/>
		<rdfs:seeAlso rdf:resource="&android-2_1;OrgApacheHttpConn"/>
		<rdfs:comment xml:lang="en">Java API part implementing the org.apache.http.impl.client package for Android 2.1</rdfs:comment>
	</owl:Class>
	<owl:Class rdf:about="&android-2_1;OrgApacheHttpImplConn">
		<owl:equivalentClass rdf:resource="&android-1_6;OrgApacheHttpImplConn"/>
		<rdfs:subClassOf rdf:resource="&java;JavaAPIPart"/>
		<rdfs:seeAlso rdf:resource="&android-2_1;OrgApacheCommonsLogging"/>
		<rdfs:seeAlso rdf:resource="&android-2_1;JavaLang"/>
		<rdfs:seeAlso rdf:resource="&android-2_1;OrgApacheHttpParams"/>
		<rdfs:seeAlso rdf:resource="&android-2_1;OrgApacheHttpConnRouting"/>
		<rdfs:seeAlso rdf:resource="&android-2_1;OrgApacheHttp"/>
		<rdfs:seeAlso rdf:resource="&android-2_1;JavaNet"/>
		<rdfs:seeAlso rdf:resource="&android-2_1;JavaUtilConcurrent"/>
		<rdfs:seeAlso rdf:resource="&android-2_1;OrgApacheHttpMessage"/>
		<rdfs:seeAlso rdf:resource="&android-2_1;OrgApacheHttpUtil"/>
		<rdfs:seeAlso rdf:resource="&android-2_1;JavaUtil"/>
		<rdfs:seeAlso rdf:resource="&android-2_1;OrgApacheHttpIo"/>
		<rdfs:seeAlso rdf:resource="&android-2_1;OrgApacheHttpConnScheme"/>
		<rdfs:seeAlso rdf:resource="&android-2_1;OrgApacheHttpProtocol"/>
		<rdfs:seeAlso rdf:resource="&android-2_1;JavaIo"/>
		<rdfs:seeAlso rdf:resource="&android-2_1;JavaxNetSsl"/>
		<rdfs:seeAlso rdf:resource="&android-2_1;OrgApacheHttpImpl"/>
		<rdfs:seeAlso rdf:resource="&android-2_1;OrgApacheHttpImplIo"/>
		<rdfs:seeAlso rdf:resource="&android-2_1;OrgApacheHttpConn"/>
		<rdfs:comment xml:lang="en">Java API part implementing the org.apache.http.impl.conn package for Android 2.1</rdfs:comment>
	</owl:Class>
	<owl:Class rdf:about="&android-2_1;OrgApacheHttpImplConnTsccm">
		<owl:equivalentClass rdf:resource="&android-1_6;OrgApacheHttpImplConnTsccm"/>
		<rdfs:subClassOf rdf:resource="&java;JavaAPIPart"/>
		<rdfs:seeAlso rdf:resource="&android-2_1;JavaUtilConcurrentLocks"/>
		<rdfs:seeAlso rdf:resource="&android-2_1;JavaLang"/>
		<rdfs:seeAlso rdf:resource="&android-2_1;JavaLangRef"/>
		<rdfs:seeAlso rdf:resource="&android-2_1;OrgApacheHttpParams"/>
		<rdfs:seeAlso rdf:resource="&android-2_1;OrgApacheHttpConnRouting"/>
		<rdfs:seeAlso rdf:resource="&android-2_1;JavaUtilConcurrent"/>
		<rdfs:seeAlso rdf:resource="&android-2_1;JavaUtil"/>
		<rdfs:seeAlso rdf:resource="&android-2_1;OrgApacheHttpConnScheme"/>
		<rdfs:seeAlso rdf:resource="&android-2_1;OrgApacheHttpImplConn"/>
		<rdfs:seeAlso rdf:resource="&android-2_1;OrgApacheHttpConn"/>
		<rdfs:comment xml:lang="en">Java API part implementing the org.apache.http.impl.conn.tsccm package for Android 2.1</rdfs:comment>
	</owl:Class>
	<owl:Class rdf:about="&android-2_1;OrgApacheHttpImplIo">
		<owl:equivalentClass rdf:resource="&android-1_6;OrgApacheHttpImplIo"/>
		<rdfs:subClassOf rdf:resource="&java;JavaAPIPart"/>
		<rdfs:seeAlso rdf:resource="&android-2_1;OrgApacheHttpMessage"/>
		<rdfs:seeAlso rdf:resource="&android-2_1;JavaLang"/>
		<rdfs:seeAlso rdf:resource="&android-2_1;OrgApacheHttpUtil"/>
		<rdfs:seeAlso rdf:resource="&android-2_1;OrgApacheHttpIo"/>
		<rdfs:seeAlso rdf:resource="&android-2_1;OrgApacheHttpParams"/>
		<rdfs:seeAlso rdf:resource="&android-2_1;JavaIo"/>
		<rdfs:seeAlso rdf:resource="&android-2_1;OrgApacheHttp"/>
		<rdfs:seeAlso rdf:resource="&android-2_1;JavaNet"/>
		<rdfs:comment xml:lang="en">Java API part implementing the org.apache.http.impl.io package for Android 2.1</rdfs:comment>
	</owl:Class>
	<owl:Class rdf:about="&android-2_1;OrgApacheHttpImplCookie">
		<owl:equivalentClass rdf:resource="&android-1_6;OrgApacheHttpImplCookie"/>
		<rdfs:subClassOf rdf:resource="&java;JavaAPIPart"/>
		<rdfs:seeAlso rdf:resource="&android-2_1;OrgApacheHttpMessage"/>
		<rdfs:seeAlso rdf:resource="&android-2_1;JavaLang"/>
		<rdfs:seeAlso rdf:resource="&android-2_1;OrgApacheHttpUtil"/>
		<rdfs:seeAlso rdf:resource="&android-2_1;JavaUtil"/>
		<rdfs:seeAlso rdf:resource="&android-2_1;OrgApacheHttpParams"/>
		<rdfs:seeAlso rdf:resource="&android-2_1;OrgApacheHttpCookie"/>
		<rdfs:seeAlso rdf:resource="&android-2_1;OrgApacheHttp"/>
		<rdfs:comment xml:lang="en">Java API part implementing the org.apache.http.impl.cookie package for Android 2.1</rdfs:comment>
	</owl:Class>
	<owl:Class rdf:about="&android-2_1;OrgApacheHttpIo">
		<owl:equivalentClass rdf:resource="&android-1_6;OrgApacheHttpIo"/>
		<rdfs:subClassOf rdf:resource="&java;JavaAPIPart"/>
		<rdfs:seeAlso rdf:resource="&android-2_1;OrgApacheHttp"/>
		<rdfs:seeAlso rdf:resource="&android-2_1;JavaLang"/>
		<rdfs:seeAlso rdf:resource="&android-2_1;OrgApacheHttpUtil"/>
		<rdfs:comment xml:lang="en">Java API part implementing the org.apache.http.io package for Android 2.1</rdfs:comment>
	</owl:Class>
	<owl:Class rdf:about="&android-2_1;OrgJson">
		<owl:equivalentClass rdf:resource="&android-1_6;OrgJson"/>
		<rdfs:subClassOf rdf:resource="&java;JavaAPIPart"/>
		<rdfs:seeAlso rdf:resource="&android-2_1;JavaLang"/>
		<rdfs:seeAlso rdf:resource="&android-2_1;JavaUtil"/>
		<rdfs:comment xml:lang="en">Java API part implementing the org.json package for Android 2.1</rdfs:comment>
	</owl:Class>
	<owl:Class rdf:about="&android-2_1;JavaxMicroeditionKhronosOpengles">
		<owl:equivalentClass rdf:resource="&android-1_6;JavaxMicroeditionKhronosOpengles"/>
		<rdfs:subClassOf rdf:resource="&java;JavaAPIPart"/>
		<rdfs:seeAlso rdf:resource="&android-2_1;JavaLang"/>
		<rdfs:seeAlso rdf:resource="&android-2_1;JavaNio"/>
		<rdfs:comment xml:lang="en">Java API part implementing the javax.microedition.khronos.opengles package for Android 2.1</rdfs:comment>
	</owl:Class>
	<owl:Class rdf:about="&android-2_1;JavaxMicroeditionKhronosEgl">
		<owl:equivalentClass rdf:resource="&android-1_6;JavaxMicroeditionKhronosEgl"/>
		<rdfs:subClassOf rdf:resource="&java;JavaAPIPart"/>
		<rdfs:seeAlso rdf:resource="&android-2_1;JavaLang"/>
		<rdfs:seeAlso rdf:resource="&android-2_1;JavaxMicroeditionKhronosOpengles"/>
		<rdfs:comment xml:lang="en">Java API part implementing the javax.microedition.khronos.egl package for Android 2.1</rdfs:comment>
	</owl:Class>
	<owl:Class rdf:about="&android-2_1;JavaxNet">
		<owl:equivalentClass rdf:resource="&java-se-6;JavaxNet"/>
		<owl:equivalentClass rdf:resource="&android-1_6;JavaxNet"/>
		<rdfs:subClassOf rdf:resource="&java;JavaAPIPart"/>
		<rdfs:seeAlso rdf:resource="&android-2_1;JavaLang"/>
		<rdfs:seeAlso rdf:resource="&android-2_1;JavaNet"/>
		<rdfs:comment xml:lang="en">Java API part implementing the javax.net package for Android 2.1</rdfs:comment>
	</owl:Class>
	<owl:Class rdf:about="&android-2_1;JavaxNetSsl">
		<owl:equivalentClass rdf:resource="&android-1_6;JavaxNetSsl"/>
		<rdfs:subClassOf rdf:resource="&java;JavaAPIPart"/>
		<rdfs:seeAlso rdf:resource="&android-2_1;JavaxNet"/>
		<rdfs:seeAlso rdf:resource="&android-2_1;JavaLang"/>
		<rdfs:seeAlso rdf:resource="&android-2_1;JavaNet"/>
		<rdfs:seeAlso rdf:resource="&android-2_1;JavaSecurityCert"/>
		<rdfs:seeAlso rdf:resource="&android-2_1;JavaUtil"/>
		<rdfs:seeAlso rdf:resource="&android-2_1;JavaIo"/>
		<rdfs:seeAlso rdf:resource="&android-2_1;JavaSecurity"/>
		<rdfs:seeAlso rdf:resource="&android-2_1;JavaNio"/>
		<rdfs:comment xml:lang="en">Java API part implementing the javax.net.ssl package for Android 2.1</rdfs:comment>
	</owl:Class>
	<owl:Class rdf:about="&android-2_1;JavaxSecurityAuth">
		<owl:equivalentClass rdf:resource="&android-1_6;JavaxSecurityAuth"/>
		<rdfs:subClassOf rdf:resource="&java;JavaAPIPart"/>
		<rdfs:seeAlso rdf:resource="&android-2_1;JavaLang"/>
		<rdfs:seeAlso rdf:resource="&android-2_1;JavaUtil"/>
		<rdfs:seeAlso rdf:resource="&android-2_1;JavaIo"/>
		<rdfs:seeAlso rdf:resource="&android-2_1;JavaSecurity"/>
		<rdfs:comment xml:lang="en">Java API part implementing the javax.security.auth package for Android 2.1</rdfs:comment>
	</owl:Class>
	<owl:Class rdf:about="&android-2_1;JavaxSecurityAuthCallback">
		<owl:equivalentClass rdf:resource="&android-1_6;JavaxSecurityAuthCallback"/>
		<rdfs:subClassOf rdf:resource="&java;JavaAPIPart"/>
		<rdfs:seeAlso rdf:resource="&android-2_1;JavaIo"/>
		<rdfs:seeAlso rdf:resource="&android-2_1;JavaLang"/>
		<rdfs:comment xml:lang="en">Java API part implementing the javax.security.auth.callback package for Android 2.1</rdfs:comment>
	</owl:Class>
	<owl:Class rdf:about="&android-2_1;JavaxSecurityAuthX500">
		<owl:equivalentClass rdf:resource="&android-1_6;JavaxSecurityAuthX500"/>
		<rdfs:subClassOf rdf:resource="&java;JavaAPIPart"/>
		<rdfs:seeAlso rdf:resource="&android-2_1;JavaIo"/>
		<rdfs:seeAlso rdf:resource="&android-2_1;JavaLang"/>
		<rdfs:seeAlso rdf:resource="&android-2_1;JavaSecurity"/>
		<rdfs:comment xml:lang="en">Java API part implementing the javax.security.auth.x500 package for Android 2.1</rdfs:comment>
	</owl:Class>
	<owl:Class rdf:about="&android-2_1;JavaxSecurityAuthLogin">
		<owl:equivalentClass rdf:resource="&android-1_6;JavaxSecurityAuthLogin"/>
		<rdfs:subClassOf rdf:resource="&java;JavaAPIPart"/>
		<rdfs:seeAlso rdf:resource="&android-2_1;JavaLang"/>
		<rdfs:seeAlso rdf:resource="&android-2_1;JavaSecurity"/>
		<rdfs:comment xml:lang="en">Java API part implementing the javax.security.auth.login package for Android 2.1</rdfs:comment>
	</owl:Class>
	<owl:Class rdf:about="&android-2_1;JavaxSecurityCert">
		<owl:equivalentClass rdf:resource="&java-se-6;JavaxSecurityCert"/>
		<owl:equivalentClass rdf:resource="&android-1_6;JavaxSecurityCert"/>
		<rdfs:subClassOf rdf:resource="&java;JavaAPIPart"/>
		<rdfs:seeAlso rdf:resource="&android-2_1;JavaIo"/>
		<rdfs:seeAlso rdf:resource="&android-2_1;JavaMath"/>
		<rdfs:seeAlso rdf:resource="&android-2_1;JavaLang"/>
		<rdfs:seeAlso rdf:resource="&android-2_1;JavaUtil"/>
		<rdfs:seeAlso rdf:resource="&android-2_1;JavaSecurity"/>
		<rdfs:comment xml:lang="en">Java API part implementing the javax.security.cert package for Android 2.1</rdfs:comment>
	</owl:Class>
	<owl:Class rdf:about="&android-2_1;JavaxCrypto">
		<owl:equivalentClass rdf:resource="&java-se-6;JavaxCrypto"/>
		<owl:equivalentClass rdf:resource="&android-1_6;JavaxCrypto"/>
		<rdfs:subClassOf rdf:resource="&java;JavaAPIPart"/>
		<rdfs:seeAlso rdf:resource="&android-2_1;JavaSecurityCert"/>
		<rdfs:seeAlso rdf:resource="&android-2_1;JavaSecuritySpec"/>
		<rdfs:seeAlso rdf:resource="&android-2_1;JavaLang"/>
		<rdfs:seeAlso rdf:resource="&android-2_1;JavaIo"/>
		<rdfs:seeAlso rdf:resource="&android-2_1;JavaNio"/>
		<rdfs:seeAlso rdf:resource="&android-2_1;JavaSecurity"/>
		<rdfs:comment xml:lang="en">Java API part implementing the javax.crypto package for Android 2.1</rdfs:comment>
	</owl:Class>
	<owl:Class rdf:about="&android-2_1;JavaxCryptoInterfaces">
		<owl:equivalentClass rdf:resource="&java-se-6;JavaxCryptoInterfaces"/>
		<owl:equivalentClass rdf:resource="&android-1_6;JavaxCryptoInterfaces"/>
		<rdfs:subClassOf rdf:resource="&java;JavaAPIPart"/>
		<rdfs:seeAlso rdf:resource="&android-2_1;JavaMath"/>
		<rdfs:seeAlso rdf:resource="&android-2_1;JavaxCrypto"/>
		<rdfs:seeAlso rdf:resource="&android-2_1;JavaxCryptoSpec"/>
		<rdfs:seeAlso rdf:resource="&android-2_1;JavaSecurity"/>
		<rdfs:comment xml:lang="en">Java API part implementing the javax.crypto.interfaces package for Android 2.1</rdfs:comment>
	</owl:Class>
	<owl:Class rdf:about="&android-2_1;JavaxCryptoSpec">
		<owl:equivalentClass rdf:resource="&java-se-6;JavaxCryptoSpec"/>
		<owl:equivalentClass rdf:resource="&android-1_6;JavaxCryptoSpec"/>
		<rdfs:subClassOf rdf:resource="&java;JavaAPIPart"/>
		<rdfs:seeAlso rdf:resource="&android-2_1;JavaIo"/>
		<rdfs:seeAlso rdf:resource="&android-2_1;JavaMath"/>
		<rdfs:seeAlso rdf:resource="&android-2_1;JavaxCrypto"/>
		<rdfs:seeAlso rdf:resource="&android-2_1;JavaSecuritySpec"/>
		<rdfs:seeAlso rdf:resource="&android-2_1;JavaLang"/>
		<rdfs:comment xml:lang="en">Java API part implementing the javax.crypto.spec package for Android 2.1</rdfs:comment>
	</owl:Class>
	<owl:Class rdf:about="&android-2_1;JavaxSql">
		<owl:equivalentClass rdf:resource="&android-1_6;JavaxSql"/>
		<rdfs:subClassOf rdf:resource="&java;JavaAPIPart"/>
		<rdfs:seeAlso rdf:resource="&android-2_1;JavaMath"/>
		<rdfs:seeAlso rdf:resource="&android-2_1;JavaSql"/>
		<rdfs:seeAlso rdf:resource="&android-2_1;JavaLang"/>
		<rdfs:seeAlso rdf:resource="&android-2_1;JavaUtil"/>
		<rdfs:seeAlso rdf:resource="&android-2_1;JavaIo"/>
		<rdfs:comment xml:lang="en">Java API part implementing the javax.sql package for Android 2.1</rdfs:comment>
	</owl:Class>
	<owl:Class rdf:about="&android-2_1;JavaxXml">
		<owl:equivalentClass rdf:resource="&android-1_6;JavaxXml"/>
		<rdfs:subClassOf rdf:resource="&java-se-6;JavaxXml"/>
		<rdfs:seeAlso rdf:resource="&android-2_1;JavaLang"/>
		<rdfs:comment xml:lang="en">Java API part implementing the javax.xml package for Android 2.1</rdfs:comment>
	</owl:Class>
	<owl:Class rdf:about="&android-2_1;JavaxXmlParsers">
		<owl:equivalentClass rdf:resource="&android-1_6;JavaxXmlParsers"/>
		<rdfs:subClassOf rdf:resource="&java;JavaAPIPart"/>
		<rdfs:seeAlso rdf:resource="&android-2_1;OrgXmlSax"/>
		<rdfs:seeAlso rdf:resource="&android-2_1;JavaLang"/>
		<rdfs:seeAlso rdf:resource="&android-2_1;OrgXmlSaxHelpers"/>
		<rdfs:seeAlso rdf:resource="&android-2_1;JavaIo"/>
		<rdfs:seeAlso rdf:resource="&android-2_1;OrgW3cDom"/>
		<rdfs:comment xml:lang="en">Java API part implementing the javax.xml.parsers package for Android 2.1</rdfs:comment>
	</owl:Class>
	<owl:Class rdf:about="&android-2_1;JunitFramework">
		<owl:equivalentClass rdf:resource="&android-1_6;JunitFramework"/>
		<rdfs:subClassOf rdf:resource="&java;JavaAPIPart"/>
		<rdfs:seeAlso rdf:resource="&android-2_1;JavaLang"/>
		<rdfs:seeAlso rdf:resource="&android-2_1;JavaUtil"/>
		<rdfs:seeAlso rdf:resource="&android-2_1;JavaLangReflect"/>
		<rdfs:comment xml:lang="en">Java API part implementing the junit.framework package for Android 2.1</rdfs:comment>
	</owl:Class>
	<owl:Class rdf:about="&android-2_1;JunitRunner">
		<owl:equivalentClass rdf:resource="&android-1_6;JunitRunner"/>
		<rdfs:subClassOf rdf:resource="&java;JavaAPIPart"/>
		<rdfs:seeAlso rdf:resource="&android-2_1;JunitFramework"/>
		<rdfs:seeAlso rdf:resource="&android-2_1;JavaLang"/>
		<rdfs:seeAlso rdf:resource="&android-2_1;JavaUtil"/>
		<rdfs:comment xml:lang="en">Java API part implementing the junit.runner package for Android 2.1</rdfs:comment>
	</owl:Class>
	<owl:Class rdf:about="&android-2_1;DalvikAnnotation">
		<owl:equivalentClass rdf:resource="&android-1_6;DalvikAnnotation"/>
		<rdfs:subClassOf rdf:resource="&java;JavaAPIPart"/>
		<rdfs:seeAlso rdf:resource="&android-2_1;JavaLangAnnotation"/>
		<rdfs:seeAlso rdf:resource="&android-2_1;JavaLang"/>
		<rdfs:comment xml:lang="en">Java API part implementing the dalvik.annotation package for Android 2.1</rdfs:comment>
	</owl:Class>
	<owl:Class rdf:about="&android-2_1;DalvikBytecode">
		<owl:equivalentClass rdf:resource="&android-1_6;DalvikBytecode"/>
		<rdfs:subClassOf rdf:resource="&java;JavaAPIPart"/>
		<rdfs:comment xml:lang="en">Java API part implementing the dalvik.bytecode package for Android 2.1</rdfs:comment>
	</owl:Class>
	<owl:Class rdf:about="&android-2_1;DalvikSystem">
		<owl:equivalentClass rdf:resource="&android-1_6;DalvikSystem"/>
		<rdfs:subClassOf rdf:resource="&java;JavaAPIPart"/>
		<rdfs:seeAlso rdf:resource="&android-2_1;JavaIo"/>
		<rdfs:seeAlso rdf:resource="&android-2_1;JavaLang"/>
		<rdfs:seeAlso rdf:resource="&android-2_1;JavaNet"/>
		<rdfs:seeAlso rdf:resource="&android-2_1;JavaUtil"/>
		<rdfs:comment xml:lang="en">Java API part implementing the dalvik.system package for Android 2.1</rdfs:comment>
	</owl:Class>
	<owl:Class rdf:about="&android-2_1;AndroidAPI">
		<rdfs:subClassOf rdf:resource="&android-1_6;AndroidAPI"/>
		<rdfs:comment xml:lang="en">JavaLibrary implementing the android package for Android 2.1</rdfs:comment>
		<rdfs:comment xml:lang="OWLManchester">platform:comprisesInterfacePart some Android</rdfs:comment>
	</owl:Class>
	<owl:Class rdf:about="&android-2_1;AndroidAccessibilityserviceAPI">
		<rdfs:subClassOf rdf:resource="&android-1_6;AndroidAccessibilityserviceAPI"/>
		<rdfs:comment xml:lang="en">JavaLibrary implementing the android.accessibilityservice package for Android 2.1</rdfs:comment>
		<rdfs:comment xml:lang="OWLManchester">platform:comprisesInterfacePart some AndroidAccessibilityservice</rdfs:comment>
	</owl:Class>
	<owl:Class rdf:about="&android-2_1;AndroidAppAPI">
		<rdfs:subClassOf rdf:resource="&android-1_6;AndroidAppAPI"/>
		<rdfs:comment xml:lang="en">JavaLibrary implementing the android.app package for Android 2.1</rdfs:comment>
		<rdfs:comment xml:lang="OWLManchester">platform:comprisesInterfacePart some AndroidApp</rdfs:comment>
	</owl:Class>
	<owl:Class rdf:about="&android-2_1;AndroidViewAPI">
		<rdfs:subClassOf rdf:resource="&java;JavaAPI"/>
		<rdfs:comment xml:lang="en">JavaLibrary implementing the android.view package for Android 2.1</rdfs:comment>
		<rdfs:comment xml:lang="OWLManchester">platform:comprisesInterfacePart some AndroidView</rdfs:comment>
	</owl:Class>
	<owl:Class rdf:about="&android-2_1;AndroidViewAccessibilityAPI">
		<owl:equivalentClass rdf:resource="&android-1_6;AndroidViewAccessibilityAPI"/>
		<rdfs:subClassOf rdf:resource="&java;JavaAPI"/>
		<rdfs:comment xml:lang="en">JavaLibrary implementing the android.view.accessibility package for Android 2.1</rdfs:comment>
		<rdfs:comment xml:lang="OWLManchester">platform:comprisesInterfacePart some AndroidViewAccessibility</rdfs:comment>
	</owl:Class>
	<owl:Class rdf:about="&android-2_1;AndroidViewInputmethodAPI">
		<rdfs:subClassOf rdf:resource="&android-1_6;AndroidViewInputmethodAPI"/>
		<rdfs:comment xml:lang="en">JavaLibrary implementing the android.view.inputmethod package for Android 2.1</rdfs:comment>
		<rdfs:comment xml:lang="OWLManchester">platform:comprisesInterfacePart some AndroidViewInputmethod</rdfs:comment>
	</owl:Class>
	<owl:Class rdf:about="&android-2_1;AndroidViewAnimationAPI">
		<rdfs:subClassOf rdf:resource="&android-1_6;AndroidViewAnimationAPI"/>
		<rdfs:comment xml:lang="en">JavaLibrary implementing the android.view.animation package for Android 2.1</rdfs:comment>
		<rdfs:comment xml:lang="OWLManchester">platform:comprisesInterfacePart some AndroidViewAnimation</rdfs:comment>
	</owl:Class>
	<owl:Class rdf:about="&android-2_1;AndroidContentAPI">
		<rdfs:subClassOf rdf:resource="&android-1_6;AndroidContentAPI"/>
		<rdfs:comment xml:lang="en">JavaLibrary implementing the android.content package for Android 2.1</rdfs:comment>
		<rdfs:comment xml:lang="OWLManchester">platform:comprisesInterfacePart some AndroidContent</rdfs:comment>
	</owl:Class>
	<owl:Class rdf:about="&android-2_1;AndroidContentResAPI">
		<rdfs:subClassOf rdf:resource="&android-1_6;AndroidContentResAPI"/>
		<rdfs:comment xml:lang="en">JavaLibrary implementing the android.content.res package for Android 2.1</rdfs:comment>
		<rdfs:comment xml:lang="OWLManchester">platform:comprisesInterfacePart some AndroidContentRes</rdfs:comment>
	</owl:Class>
	<owl:Class rdf:about="&android-2_1;AndroidContentPmAPI">
		<rdfs:subClassOf rdf:resource="&android-1_6;AndroidContentPmAPI"/>
		<rdfs:comment xml:lang="en">JavaLibrary implementing the android.content.pm package for Android 2.1</rdfs:comment>
		<rdfs:comment xml:lang="OWLManchester">platform:comprisesInterfacePart some AndroidContentPm</rdfs:comment>
	</owl:Class>
	<owl:Class rdf:about="&android-2_1;AndroidOsAPI">
		<rdfs:subClassOf rdf:resource="&android-1_6;AndroidOsAPI"/>
		<rdfs:comment xml:lang="en">JavaLibrary implementing the android.os package for Android 2.1</rdfs:comment>
		<rdfs:comment xml:lang="OWLManchester">platform:comprisesInterfacePart some AndroidOs</rdfs:comment>
	</owl:Class>
	<owl:Class rdf:about="&android-2_1;AndroidAccountsAPI">
		<rdfs:subClassOf rdf:resource="&java;JavaAPI"/>
		<rdfs:comment xml:lang="en">JavaLibrary implementing the android.accounts package for Android 2.1</rdfs:comment>
		<rdfs:comment xml:lang="OWLManchester">platform:comprisesInterfacePart some AndroidAccounts</rdfs:comment>
	</owl:Class>
	<owl:Class rdf:about="&android-2_1;AndroidGraphicsAPI">
		<rdfs:subClassOf rdf:resource="&android-1_6;AndroidGraphicsAPI"/>
		<rdfs:comment xml:lang="en">JavaLibrary implementing the android.graphics package for Android 2.1</rdfs:comment>
		<rdfs:comment xml:lang="OWLManchester">platform:comprisesInterfacePart some AndroidGraphics</rdfs:comment>
	</owl:Class>
	<owl:Class rdf:about="&android-2_1;AndroidGraphicsDrawableAPI">
		<rdfs:subClassOf rdf:resource="&android-1_6;AndroidGraphicsDrawableAPI"/>
		<rdfs:comment xml:lang="en">JavaLibrary implementing the android.graphics.drawable package for Android 2.1</rdfs:comment>
		<rdfs:comment xml:lang="OWLManchester">platform:comprisesInterfacePart some AndroidGraphicsDrawable</rdfs:comment>
	</owl:Class>
	<owl:Class rdf:about="&android-2_1;AndroidGraphicsDrawableShapesAPI">
		<owl:equivalentClass rdf:resource="&android-1_6;AndroidGraphicsDrawableShapesAPI"/>
		<rdfs:subClassOf rdf:resource="&java;JavaAPI"/>
		<rdfs:comment xml:lang="en">JavaLibrary implementing the android.graphics.drawable.shapes package for Android 2.1</rdfs:comment>
		<rdfs:comment xml:lang="OWLManchester">platform:comprisesInterfacePart some AndroidGraphicsDrawableShapes</rdfs:comment>
	</owl:Class>
	<owl:Class rdf:about="&android-2_1;AndroidNetAPI">
		<owl:equivalentClass rdf:resource="&android-1_6;AndroidNetAPI"/>
		<rdfs:subClassOf rdf:resource="&java;JavaAPI"/>
		<rdfs:comment xml:lang="en">JavaLibrary implementing the android.net package for Android 2.1</rdfs:comment>
		<rdfs:comment xml:lang="OWLManchester">platform:comprisesInterfacePart some AndroidNet</rdfs:comment>
	</owl:Class>
	<owl:Class rdf:about="&android-2_1;AndroidNetHttpAPI">
		<owl:equivalentClass rdf:resource="&android-1_6;AndroidNetHttpAPI"/>
		<rdfs:subClassOf rdf:resource="&java;JavaAPI"/>
		<rdfs:comment xml:lang="en">JavaLibrary implementing the android.net.http package for Android 2.1</rdfs:comment>
		<rdfs:comment xml:lang="OWLManchester">platform:comprisesInterfacePart some AndroidNetHttp</rdfs:comment>
	</owl:Class>
	<owl:Class rdf:about="&android-2_1;AndroidNetWifiAPI">
		<owl:equivalentClass rdf:resource="&android-1_6;AndroidNetWifiAPI"/>
		<rdfs:subClassOf rdf:resource="&java;JavaAPI"/>
		<rdfs:comment xml:lang="en">JavaLibrary implementing the android.net.wifi package for Android 2.1</rdfs:comment>
		<rdfs:comment xml:lang="OWLManchester">platform:comprisesInterfacePart some AndroidNetWifi</rdfs:comment>
	</owl:Class>
	<owl:Class rdf:about="&android-2_1;AndroidDatabaseAPI">
		<rdfs:subClassOf rdf:resource="&android-1_6;AndroidDatabaseAPI"/>
		<rdfs:comment xml:lang="en">JavaLibrary implementing the android.database package for Android 2.1</rdfs:comment>
		<rdfs:comment xml:lang="OWLManchester">platform:comprisesInterfacePart some AndroidDatabase</rdfs:comment>
	</owl:Class>
	<owl:Class rdf:about="&android-2_1;AndroidDatabaseSqliteAPI">
		<rdfs:subClassOf rdf:resource="&android-1_6;AndroidDatabaseSqliteAPI"/>
		<rdfs:comment xml:lang="en">JavaLibrary implementing the android.database.sqlite package for Android 2.1</rdfs:comment>
		<rdfs:comment xml:lang="OWLManchester">platform:comprisesInterfacePart some AndroidDatabaseSqlite</rdfs:comment>
	</owl:Class>
	<owl:Class rdf:about="&android-2_1;AndroidUtilAPI">
		<rdfs:subClassOf rdf:resource="&android-1_6;AndroidUtilAPI"/>
		<rdfs:comment xml:lang="en">JavaLibrary implementing the android.util package for Android 2.1</rdfs:comment>
		<rdfs:comment xml:lang="OWLManchester">platform:comprisesInterfacePart some AndroidUtil</rdfs:comment>
	</owl:Class>
	<owl:Class rdf:about="&android-2_1;AndroidWidgetAPI">
		<rdfs:subClassOf rdf:resource="&java;JavaAPI"/>
		<rdfs:comment xml:lang="en">JavaLibrary implementing the android.widget package for Android 2.1</rdfs:comment>
		<rdfs:comment xml:lang="OWLManchester">platform:comprisesInterfacePart some AndroidWidget</rdfs:comment>
	</owl:Class>
	<owl:Class rdf:about="&android-2_1;AndroidAppwidgetAPI">
		<rdfs:subClassOf rdf:resource="&java;JavaAPI"/>
		<rdfs:comment xml:lang="en">JavaLibrary implementing the android.appwidget package for Android 2.1</rdfs:comment>
		<rdfs:comment xml:lang="OWLManchester">platform:comprisesInterfacePart some AndroidAppwidget</rdfs:comment>
	</owl:Class>
	<owl:Class rdf:about="&android-2_1;AndroidBluetoothAPI">
		<rdfs:subClassOf rdf:resource="&java;JavaAPI"/>
		<rdfs:comment xml:lang="en">JavaLibrary implementing the android.bluetooth package for Android 2.1</rdfs:comment>
		<rdfs:comment xml:lang="OWLManchester">platform:comprisesInterfacePart some AndroidBluetooth</rdfs:comment>
	</owl:Class>
	<owl:Class rdf:about="&android-2_1;AndroidGestureAPI">
		<rdfs:subClassOf rdf:resource="&java;JavaAPI"/>
		<rdfs:comment xml:lang="en">JavaLibrary implementing the android.gesture package for Android 2.1</rdfs:comment>
		<rdfs:comment xml:lang="OWLManchester">platform:comprisesInterfacePart some AndroidGesture</rdfs:comment>
	</owl:Class>
	<owl:Class rdf:about="&android-2_1;AndroidHardwareAPI">
		<rdfs:subClassOf rdf:resource="&android-1_6;AndroidHardwareAPI"/>
		<rdfs:comment xml:lang="en">JavaLibrary implementing the android.hardware package for Android 2.1</rdfs:comment>
		<rdfs:comment xml:lang="OWLManchester">platform:comprisesInterfacePart some AndroidHardware</rdfs:comment>
	</owl:Class>
	<owl:Class rdf:about="&android-2_1;AndroidInputmethodserviceAPI">
		<rdfs:subClassOf rdf:resource="&android-1_6;AndroidInputmethodserviceAPI"/>
		<rdfs:comment xml:lang="en">JavaLibrary implementing the android.inputmethodservice package for Android 2.1</rdfs:comment>
		<rdfs:comment xml:lang="OWLManchester">platform:comprisesInterfacePart some AndroidInputmethodservice</rdfs:comment>
	</owl:Class>
	<owl:Class rdf:about="&android-2_1;AndroidLocationAPI">
		<rdfs:subClassOf rdf:resource="&android-1_6;AndroidLocationAPI"/>
		<rdfs:comment xml:lang="en">JavaLibrary implementing the android.location package for Android 2.1</rdfs:comment>
		<rdfs:comment xml:lang="OWLManchester">platform:comprisesInterfacePart some AndroidLocation</rdfs:comment>
	</owl:Class>
	<owl:Class rdf:about="&android-2_1;AndroidMediaAPI">
		<rdfs:subClassOf rdf:resource="&android-1_6;AndroidMediaAPI"/>
		<rdfs:comment xml:lang="en">JavaLibrary implementing the android.media package for Android 2.1</rdfs:comment>
		<rdfs:comment xml:lang="OWLManchester">platform:comprisesInterfacePart some AndroidMedia</rdfs:comment>
	</owl:Class>
	<owl:Class rdf:about="&android-2_1;AndroidOpenglAPI">
		<rdfs:subClassOf rdf:resource="&android-1_6;AndroidOpenglAPI"/>
		<rdfs:comment xml:lang="en">JavaLibrary implementing the android.opengl package for Android 2.1</rdfs:comment>
		<rdfs:comment xml:lang="OWLManchester">platform:comprisesInterfacePart some AndroidOpengl</rdfs:comment>
	</owl:Class>
	<owl:Class rdf:about="&android-2_1;AndroidPreferenceAPI">
		<rdfs:subClassOf rdf:resource="&android-1_6;AndroidPreferenceAPI"/>
		<rdfs:comment xml:lang="en">JavaLibrary implementing the android.preference package for Android 2.1</rdfs:comment>
		<rdfs:comment xml:lang="OWLManchester">platform:comprisesInterfacePart some AndroidPreference</rdfs:comment>
	</owl:Class>
	<owl:Class rdf:about="&android-2_1;AndroidProviderAPI">
		<rdfs:subClassOf rdf:resource="&android-1_6;AndroidProviderAPI"/>
		<rdfs:comment xml:lang="en">JavaLibrary implementing the android.provider package for Android 2.1</rdfs:comment>
		<rdfs:comment xml:lang="OWLManchester">platform:comprisesInterfacePart some AndroidProvider</rdfs:comment>
	</owl:Class>
	<owl:Class rdf:about="&android-2_1;AndroidWebkitAPI">
		<rdfs:subClassOf rdf:resource="&java;JavaAPI"/>
		<rdfs:comment xml:lang="en">JavaLibrary implementing the android.webkit package for Android 2.1</rdfs:comment>
		<rdfs:comment xml:lang="OWLManchester">platform:comprisesInterfacePart some AndroidWebkit</rdfs:comment>
	</owl:Class>
	<owl:Class rdf:about="&android-2_1;AndroidSaxAPI">
		<owl:equivalentClass rdf:resource="&android-1_6;AndroidSaxAPI"/>
		<rdfs:subClassOf rdf:resource="&java;JavaAPI"/>
		<rdfs:comment xml:lang="en">JavaLibrary implementing the android.sax package for Android 2.1</rdfs:comment>
		<rdfs:comment xml:lang="OWLManchester">platform:comprisesInterfacePart some AndroidSax</rdfs:comment>
	</owl:Class>
	<owl:Class rdf:about="&android-2_1;AndroidServiceWallpaperAPI">
		<rdfs:subClassOf rdf:resource="&java;JavaAPI"/>
		<rdfs:comment xml:lang="en">JavaLibrary implementing the android.service.wallpaper package for Android 2.1</rdfs:comment>
		<rdfs:comment xml:lang="OWLManchester">platform:comprisesInterfacePart some AndroidServiceWallpaper</rdfs:comment>
	</owl:Class>
	<owl:Class rdf:about="&android-2_1;AndroidSpeechAPI">
		<owl:equivalentClass rdf:resource="&android-1_6;AndroidSpeechAPI"/>
		<rdfs:subClassOf rdf:resource="&java;JavaAPI"/>
		<rdfs:comment xml:lang="en">JavaLibrary implementing the android.speech package for Android 2.1</rdfs:comment>
		<rdfs:comment xml:lang="OWLManchester">platform:comprisesInterfacePart some AndroidSpeech</rdfs:comment>
	</owl:Class>
	<owl:Class rdf:about="&android-2_1;AndroidSpeechTtsAPI">
		<owl:equivalentClass rdf:resource="&android-1_6;AndroidSpeechTtsAPI"/>
		<rdfs:subClassOf rdf:resource="&java;JavaAPI"/>
		<rdfs:comment xml:lang="en">JavaLibrary implementing the android.speech.tts package for Android 2.1</rdfs:comment>
		<rdfs:comment xml:lang="OWLManchester">platform:comprisesInterfacePart some AndroidSpeechTts</rdfs:comment>
	</owl:Class>
	<owl:Class rdf:about="&android-2_1;AndroidTelephonyAPI">
		<rdfs:subClassOf rdf:resource="&android-1_6;AndroidTelephonyAPI"/>
		<rdfs:comment xml:lang="en">JavaLibrary implementing the android.telephony package for Android 2.1</rdfs:comment>
		<rdfs:comment xml:lang="OWLManchester">platform:comprisesInterfacePart some AndroidTelephony</rdfs:comment>
	</owl:Class>
	<owl:Class rdf:about="&android-2_1;AndroidTelephonyCdmaAPI">
		<rdfs:subClassOf rdf:resource="&java;JavaAPI"/>
		<rdfs:comment xml:lang="en">JavaLibrary implementing the android.telephony.cdma package for Android 2.1</rdfs:comment>
		<rdfs:comment xml:lang="OWLManchester">platform:comprisesInterfacePart some AndroidTelephonyCdma</rdfs:comment>
	</owl:Class>
	<owl:Class rdf:about="&android-2_1;AndroidTelephonyGsmAPI">
		<owl:equivalentClass rdf:resource="&android-1_6;AndroidTelephonyGsmAPI"/>
		<rdfs:subClassOf rdf:resource="&java;JavaAPI"/>
		<rdfs:comment xml:lang="en">JavaLibrary implementing the android.telephony.gsm package for Android 2.1</rdfs:comment>
		<rdfs:comment xml:lang="OWLManchester">platform:comprisesInterfacePart some AndroidTelephonyGsm</rdfs:comment>
	</owl:Class>
	<owl:Class rdf:about="&android-2_1;AndroidTextAPI">
		<rdfs:subClassOf rdf:resource="&android-1_6;AndroidTextAPI"/>
		<rdfs:comment xml:lang="en">JavaLibrary implementing the android.text package for Android 2.1</rdfs:comment>
		<rdfs:comment xml:lang="OWLManchester">platform:comprisesInterfacePart some AndroidText</rdfs:comment>
	</owl:Class>
	<owl:Class rdf:about="&android-2_1;AndroidTextFormatAPI">
		<rdfs:subClassOf rdf:resource="&android-1_6;AndroidTextFormatAPI"/>
		<rdfs:comment xml:lang="en">JavaLibrary implementing the android.text.format package for Android 2.1</rdfs:comment>
		<rdfs:comment xml:lang="OWLManchester">platform:comprisesInterfacePart some AndroidTextFormat</rdfs:comment>
	</owl:Class>
	<owl:Class rdf:about="&android-2_1;AndroidTextMethodAPI">
		<rdfs:subClassOf rdf:resource="&android-1_6;AndroidTextMethodAPI"/>
		<rdfs:comment xml:lang="en">JavaLibrary implementing the android.text.method package for Android 2.1</rdfs:comment>
		<rdfs:comment xml:lang="OWLManchester">platform:comprisesInterfacePart some AndroidTextMethod</rdfs:comment>
	</owl:Class>
	<owl:Class rdf:about="&android-2_1;AndroidTextStyleAPI">
		<rdfs:subClassOf rdf:resource="&android-1_6;AndroidTextStyleAPI"/>
		<rdfs:comment xml:lang="en">JavaLibrary implementing the android.text.style package for Android 2.1</rdfs:comment>
		<rdfs:comment xml:lang="OWLManchester">platform:comprisesInterfacePart some AndroidTextStyle</rdfs:comment>
	</owl:Class>
	<owl:Class rdf:about="&android-2_1;AndroidTextUtilAPI">
		<owl:equivalentClass rdf:resource="&android-1_6;AndroidTextUtilAPI"/>
		<rdfs:subClassOf rdf:resource="&java;JavaAPI"/>
		<rdfs:comment xml:lang="en">JavaLibrary implementing the android.text.util package for Android 2.1</rdfs:comment>
		<rdfs:comment xml:lang="OWLManchester">platform:comprisesInterfacePart some AndroidTextUtil</rdfs:comment>
	</owl:Class>
	<owl:Class rdf:about="&android-2_1;AndroidTestAPI">
		<rdfs:subClassOf rdf:resource="&android-1_6;AndroidTestAPI"/>
		<rdfs:comment xml:lang="en">JavaLibrary implementing the android.test package for Android 2.1</rdfs:comment>
		<rdfs:comment xml:lang="OWLManchester">platform:comprisesInterfacePart some AndroidTest</rdfs:comment>
	</owl:Class>
	<owl:Class rdf:about="&android-2_1;AndroidTestMockAPI">
		<rdfs:subClassOf rdf:resource="&android-1_6;AndroidTestMockAPI"/>
		<rdfs:comment xml:lang="en">JavaLibrary implementing the android.test.mock package for Android 2.1</rdfs:comment>
		<rdfs:comment xml:lang="OWLManchester">platform:comprisesInterfacePart some AndroidTestMock</rdfs:comment>
	</owl:Class>
	<owl:Class rdf:about="&android-2_1;AndroidTestSuitebuilderAPI">
		<owl:equivalentClass rdf:resource="&android-1_6;AndroidTestSuitebuilderAPI"/>
		<rdfs:subClassOf rdf:resource="&java;JavaAPI"/>
		<rdfs:comment xml:lang="en">JavaLibrary implementing the android.test.suitebuilder package for Android 2.1</rdfs:comment>
		<rdfs:comment xml:lang="OWLManchester">platform:comprisesInterfacePart some AndroidTestSuitebuilder</rdfs:comment>
	</owl:Class>
	<owl:Class rdf:about="&android-2_1;AndroidTestSuitebuilderAnnotationAPI">
		<owl:equivalentClass rdf:resource="&android-1_6;AndroidTestSuitebuilderAnnotationAPI"/>
		<rdfs:subClassOf rdf:resource="&java;JavaAPI"/>
		<rdfs:comment xml:lang="en">JavaLibrary implementing the android.test.suitebuilder.annotation package for Android 2.1</rdfs:comment>
		<rdfs:comment xml:lang="OWLManchester">platform:comprisesInterfacePart some AndroidTestSuitebuilderAnnotation</rdfs:comment>
	</owl:Class>
	<owl:Class rdf:about="&android-2_1;JavaLangAPI">
		<owl:equivalentClass rdf:resource="&android-1_6;JavaLangAPI"/>
		<rdfs:subClassOf rdf:resource="&java;JavaAPI"/>
		<rdfs:comment xml:lang="en">JavaLibrary implementing the java.lang package for Android 2.1</rdfs:comment>
		<rdfs:comment xml:lang="OWLManchester">platform:comprisesInterfacePart some JavaLang</rdfs:comment>
	</owl:Class>
	<owl:Class rdf:about="&android-2_1;JavaLangAnnotationAPI">
		<owl:equivalentClass rdf:resource="&android-1_6;JavaLangAnnotationAPI"/>
		<rdfs:subClassOf rdf:resource="&java;JavaAPI"/>
		<rdfs:comment xml:lang="en">JavaLibrary implementing the java.lang.annotation package for Android 2.1</rdfs:comment>
		<rdfs:comment xml:lang="OWLManchester">platform:comprisesInterfacePart some JavaLangAnnotation</rdfs:comment>
	</owl:Class>
	<owl:Class rdf:about="&android-2_1;JavaLangReflectAPI">
		<owl:equivalentClass rdf:resource="&java-se-6;JavaLangReflectAPI"/>
		<owl:equivalentClass rdf:resource="&android-1_6;JavaLangReflectAPI"/>
		<rdfs:subClassOf rdf:resource="&java;JavaAPI"/>
		<rdfs:comment xml:lang="en">JavaLibrary implementing the java.lang.reflect package for Android 2.1</rdfs:comment>
		<rdfs:comment xml:lang="OWLManchester">platform:comprisesInterfacePart some JavaLangReflect</rdfs:comment>
	</owl:Class>
	<owl:Class rdf:about="&android-2_1;JavaLangRefAPI">
		<owl:equivalentClass rdf:resource="&java-se-6;JavaLangRefAPI"/>
		<owl:equivalentClass rdf:resource="&android-1_6;JavaLangRefAPI"/>
		<rdfs:subClassOf rdf:resource="&java;JavaAPI"/>
		<rdfs:comment xml:lang="en">JavaLibrary implementing the java.lang.ref package for Android 2.1</rdfs:comment>
		<rdfs:comment xml:lang="OWLManchester">platform:comprisesInterfacePart some JavaLangRef</rdfs:comment>
	</owl:Class>
	<owl:Class rdf:about="&android-2_1;JavaUtilAPI">
		<owl:equivalentClass rdf:resource="&android-1_6;JavaUtilAPI"/>
		<rdfs:subClassOf rdf:resource="&java;JavaAPI"/>
		<rdfs:comment xml:lang="en">JavaLibrary implementing the java.util package for Android 2.1</rdfs:comment>
		<rdfs:comment xml:lang="OWLManchester">platform:comprisesInterfacePart some JavaUtil</rdfs:comment>
	</owl:Class>
	<owl:Class rdf:about="&android-2_1;JavaUtilConcurrentAPI">
		<owl:equivalentClass rdf:resource="&android-1_6;JavaUtilConcurrentAPI"/>
		<rdfs:subClassOf rdf:resource="&java;JavaAPI"/>
		<rdfs:comment xml:lang="en">JavaLibrary implementing the java.util.concurrent package for Android 2.1</rdfs:comment>
		<rdfs:comment xml:lang="OWLManchester">platform:comprisesInterfacePart some JavaUtilConcurrent</rdfs:comment>
	</owl:Class>
	<owl:Class rdf:about="&android-2_1;JavaUtilConcurrentAtomicAPI">
		<owl:equivalentClass rdf:resource="&android-1_6;JavaUtilConcurrentAtomicAPI"/>
		<rdfs:subClassOf rdf:resource="&java;JavaAPI"/>
		<rdfs:comment xml:lang="en">JavaLibrary implementing the java.util.concurrent.atomic package for Android 2.1</rdfs:comment>
		<rdfs:comment xml:lang="OWLManchester">platform:comprisesInterfacePart some JavaUtilConcurrentAtomic</rdfs:comment>
	</owl:Class>
	<owl:Class rdf:about="&android-2_1;JavaUtilConcurrentLocksAPI">
		<rdfs:subClassOf rdf:resource="&android-1_6;JavaUtilConcurrentLocksAPI"/>
		<rdfs:comment xml:lang="en">JavaLibrary implementing the java.util.concurrent.locks package for Android 2.1</rdfs:comment>
		<rdfs:comment xml:lang="OWLManchester">platform:comprisesInterfacePart some JavaUtilConcurrentLocks</rdfs:comment>
	</owl:Class>
	<owl:Class rdf:about="&android-2_1;JavaUtilRegexAPI">
		<owl:equivalentClass rdf:resource="&java-se-6;JavaUtilRegexAPI"/>
		<owl:equivalentClass rdf:resource="&android-1_6;JavaUtilRegexAPI"/>
		<rdfs:subClassOf rdf:resource="&java;JavaAPI"/>
		<rdfs:comment xml:lang="en">JavaLibrary implementing the java.util.regex package for Android 2.1</rdfs:comment>
		<rdfs:comment xml:lang="OWLManchester">platform:comprisesInterfacePart some JavaUtilRegex</rdfs:comment>
	</owl:Class>
	<owl:Class rdf:about="&android-2_1;JavaUtilJarAPI">
		<owl:equivalentClass rdf:resource="&java-se-6;JavaUtilJarAPI"/>
		<owl:equivalentClass rdf:resource="&android-1_6;JavaUtilJarAPI"/>
		<rdfs:subClassOf rdf:resource="&java;JavaAPI"/>
		<rdfs:comment xml:lang="en">JavaLibrary implementing the java.util.jar package for Android 2.1</rdfs:comment>
		<rdfs:comment xml:lang="OWLManchester">platform:comprisesInterfacePart some JavaUtilJar</rdfs:comment>
	</owl:Class>
	<owl:Class rdf:about="&android-2_1;JavaUtilZipAPI">
		<owl:equivalentClass rdf:resource="&android-1_6;JavaUtilZipAPI"/>
		<rdfs:subClassOf rdf:resource="&java;JavaAPI"/>
		<rdfs:comment xml:lang="en">JavaLibrary implementing the java.util.zip package for Android 2.1</rdfs:comment>
		<rdfs:comment xml:lang="OWLManchester">platform:comprisesInterfacePart some JavaUtilZip</rdfs:comment>
	</owl:Class>
	<owl:Class rdf:about="&android-2_1;JavaUtilLoggingAPI">
		<owl:equivalentClass rdf:resource="&android-1_6;JavaUtilLoggingAPI"/>
		<rdfs:subClassOf rdf:resource="&java;JavaAPI"/>
		<rdfs:comment xml:lang="en">JavaLibrary implementing the java.util.logging package for Android 2.1</rdfs:comment>
		<rdfs:comment xml:lang="OWLManchester">platform:comprisesInterfacePart some JavaUtilLogging</rdfs:comment>
	</owl:Class>
	<owl:Class rdf:about="&android-2_1;JavaUtilPrefsAPI">
		<owl:equivalentClass rdf:resource="&java-se-6;JavaUtilPrefsAPI"/>
		<owl:equivalentClass rdf:resource="&android-1_6;JavaUtilPrefsAPI"/>
		<rdfs:subClassOf rdf:resource="&java;JavaAPI"/>
		<rdfs:comment xml:lang="en">JavaLibrary implementing the java.util.prefs package for Android 2.1</rdfs:comment>
		<rdfs:comment xml:lang="OWLManchester">platform:comprisesInterfacePart some JavaUtilPrefs</rdfs:comment>
	</owl:Class>
	<owl:Class rdf:about="&android-2_1;JavaIoAPI">
		<owl:equivalentClass rdf:resource="&android-1_6;JavaIoAPI"/>
		<rdfs:subClassOf rdf:resource="&java;JavaAPI"/>
		<rdfs:comment xml:lang="en">JavaLibrary implementing the java.io package for Android 2.1</rdfs:comment>
		<rdfs:comment xml:lang="OWLManchester">platform:comprisesInterfacePart some JavaIo</rdfs:comment>
	</owl:Class>
	<owl:Class rdf:about="&android-2_1;JavaNioAPI">
		<owl:equivalentClass rdf:resource="&android-1_6;JavaNioAPI"/>
		<rdfs:subClassOf rdf:resource="&java;JavaAPI"/>
		<rdfs:comment xml:lang="en">JavaLibrary implementing the java.nio package for Android 2.1</rdfs:comment>
		<rdfs:comment xml:lang="OWLManchester">platform:comprisesInterfacePart some JavaNio</rdfs:comment>
	</owl:Class>
	<owl:Class rdf:about="&android-2_1;JavaNioChannelsAPI">
		<owl:equivalentClass rdf:resource="&java-se-6;JavaNioChannelsAPI"/>
		<owl:equivalentClass rdf:resource="&android-1_6;JavaNioChannelsAPI"/>
		<rdfs:subClassOf rdf:resource="&java;JavaAPI"/>
		<rdfs:comment xml:lang="en">JavaLibrary implementing the java.nio.channels package for Android 2.1</rdfs:comment>
		<rdfs:comment xml:lang="OWLManchester">platform:comprisesInterfacePart some JavaNioChannels</rdfs:comment>
	</owl:Class>
	<owl:Class rdf:about="&android-2_1;JavaNioChannelsSpiAPI">
		<owl:equivalentClass rdf:resource="&java-se-6;JavaNioChannelsSpiAPI"/>
		<owl:equivalentClass rdf:resource="&android-1_6;JavaNioChannelsSpiAPI"/>
		<rdfs:subClassOf rdf:resource="&java;JavaAPI"/>
		<rdfs:comment xml:lang="en">JavaLibrary implementing the java.nio.channels.spi package for Android 2.1</rdfs:comment>
		<rdfs:comment xml:lang="OWLManchester">platform:comprisesInterfacePart some JavaNioChannelsSpi</rdfs:comment>
	</owl:Class>
	<owl:Class rdf:about="&android-2_1;JavaNioCharsetAPI">
		<owl:equivalentClass rdf:resource="&java-se-6;JavaNioCharsetAPI"/>
		<owl:equivalentClass rdf:resource="&android-1_6;JavaNioCharsetAPI"/>
		<rdfs:subClassOf rdf:resource="&java;JavaAPI"/>
		<rdfs:comment xml:lang="en">JavaLibrary implementing the java.nio.charset package for Android 2.1</rdfs:comment>
		<rdfs:comment xml:lang="OWLManchester">platform:comprisesInterfacePart some JavaNioCharset</rdfs:comment>
	</owl:Class>
	<owl:Class rdf:about="&android-2_1;JavaNioCharsetSpiAPI">
		<owl:equivalentClass rdf:resource="&java-se-6;JavaNioCharsetSpiAPI"/>
		<owl:equivalentClass rdf:resource="&android-1_6;JavaNioCharsetSpiAPI"/>
		<rdfs:subClassOf rdf:resource="&java;JavaAPI"/>
		<rdfs:comment xml:lang="en">JavaLibrary implementing the java.nio.charset.spi package for Android 2.1</rdfs:comment>
		<rdfs:comment xml:lang="OWLManchester">platform:comprisesInterfacePart some JavaNioCharsetSpi</rdfs:comment>
	</owl:Class>
	<owl:Class rdf:about="&android-2_1;JavaNetAPI">
		<owl:equivalentClass rdf:resource="&android-1_6;JavaNetAPI"/>
		<rdfs:subClassOf rdf:resource="&java;JavaAPI"/>
		<rdfs:comment xml:lang="en">JavaLibrary implementing the java.net package for Android 2.1</rdfs:comment>
		<rdfs:comment xml:lang="OWLManchester">platform:comprisesInterfacePart some JavaNet</rdfs:comment>
	</owl:Class>
	<owl:Class rdf:about="&android-2_1;JavaSecurityAPI">
		<owl:equivalentClass rdf:resource="&android-1_6;JavaSecurityAPI"/>
		<rdfs:subClassOf rdf:resource="&java;JavaAPI"/>
		<rdfs:comment xml:lang="en">JavaLibrary implementing the java.security package for Android 2.1</rdfs:comment>
		<rdfs:comment xml:lang="OWLManchester">platform:comprisesInterfacePart some JavaSecurity</rdfs:comment>
	</owl:Class>
	<owl:Class rdf:about="&android-2_1;JavaSecurityCertAPI">
		<owl:equivalentClass rdf:resource="&java-se-6;JavaSecurityCertAPI"/>
		<owl:equivalentClass rdf:resource="&android-1_6;JavaSecurityCertAPI"/>
		<rdfs:subClassOf rdf:resource="&java;JavaAPI"/>
		<rdfs:comment xml:lang="en">JavaLibrary implementing the java.security.cert package for Android 2.1</rdfs:comment>
		<rdfs:comment xml:lang="OWLManchester">platform:comprisesInterfacePart some JavaSecurityCert</rdfs:comment>
	</owl:Class>
	<owl:Class rdf:about="&android-2_1;JavaSecuritySpecAPI">
		<owl:equivalentClass rdf:resource="&java-se-6;JavaSecuritySpecAPI"/>
		<owl:equivalentClass rdf:resource="&android-1_6;JavaSecuritySpecAPI"/>
		<rdfs:subClassOf rdf:resource="&java;JavaAPI"/>
		<rdfs:comment xml:lang="en">JavaLibrary implementing the java.security.spec package for Android 2.1</rdfs:comment>
		<rdfs:comment xml:lang="OWLManchester">platform:comprisesInterfacePart some JavaSecuritySpec</rdfs:comment>
	</owl:Class>
	<owl:Class rdf:about="&android-2_1;JavaSecurityAclAPI">
		<owl:equivalentClass rdf:resource="&java-se-6;JavaSecurityAclAPI"/>
		<owl:equivalentClass rdf:resource="&android-1_6;JavaSecurityAclAPI"/>
		<rdfs:subClassOf rdf:resource="&java;JavaAPI"/>
		<rdfs:comment xml:lang="en">JavaLibrary implementing the java.security.acl package for Android 2.1</rdfs:comment>
		<rdfs:comment xml:lang="OWLManchester">platform:comprisesInterfacePart some JavaSecurityAcl</rdfs:comment>
	</owl:Class>
	<owl:Class rdf:about="&android-2_1;JavaSecurityInterfacesAPI">
		<owl:equivalentClass rdf:resource="&java-se-6;JavaSecurityInterfacesAPI"/>
		<owl:equivalentClass rdf:resource="&android-1_6;JavaSecurityInterfacesAPI"/>
		<rdfs:subClassOf rdf:resource="&java;JavaAPI"/>
		<rdfs:comment xml:lang="en">JavaLibrary implementing the java.security.interfaces package for Android 2.1</rdfs:comment>
		<rdfs:comment xml:lang="OWLManchester">platform:comprisesInterfacePart some JavaSecurityInterfaces</rdfs:comment>
	</owl:Class>
	<owl:Class rdf:about="&android-2_1;JavaTextAPI">
		<owl:equivalentClass rdf:resource="&android-1_6;JavaTextAPI"/>
		<rdfs:subClassOf rdf:resource="&java;JavaAPI"/>
		<rdfs:comment xml:lang="en">JavaLibrary implementing the java.text package for Android 2.1</rdfs:comment>
		<rdfs:comment xml:lang="OWLManchester">platform:comprisesInterfacePart some JavaText</rdfs:comment>
	</owl:Class>
	<owl:Class rdf:about="&android-2_1;JavaAwtFontAPI">
		<owl:equivalentClass rdf:resource="&android-1_6;JavaAwtFontAPI"/>
		<rdfs:subClassOf rdf:resource="&java;JavaAPI"/>
		<rdfs:comment xml:lang="en">JavaLibrary implementing the java.awt.font package for Android 2.1</rdfs:comment>
		<rdfs:comment xml:lang="OWLManchester">platform:comprisesInterfacePart some JavaAwtFont</rdfs:comment>
	</owl:Class>
	<owl:Class rdf:about="&android-2_1;JavaBeansAPI">
		<owl:equivalentClass rdf:resource="&android-1_6;JavaBeansAPI"/>
		<rdfs:subClassOf rdf:resource="&java;JavaAPI"/>
		<rdfs:comment xml:lang="en">JavaLibrary implementing the java.beans package for Android 2.1</rdfs:comment>
		<rdfs:comment xml:lang="OWLManchester">platform:comprisesInterfacePart some JavaBeans</rdfs:comment>
	</owl:Class>
	<owl:Class rdf:about="&android-2_1;JavaMathAPI">
		<owl:equivalentClass rdf:resource="&android-1_6;JavaMathAPI"/>
		<rdfs:subClassOf rdf:resource="&java;JavaAPI"/>
		<rdfs:comment xml:lang="en">JavaLibrary implementing the java.math package for Android 2.1</rdfs:comment>
		<rdfs:comment xml:lang="OWLManchester">platform:comprisesInterfacePart some JavaMath</rdfs:comment>
	</owl:Class>
	<owl:Class rdf:about="&android-2_1;JavaSqlAPI">
		<owl:equivalentClass rdf:resource="&android-1_6;JavaSqlAPI"/>
		<rdfs:subClassOf rdf:resource="&java;JavaAPI"/>
		<rdfs:comment xml:lang="en">JavaLibrary implementing the java.sql package for Android 2.1</rdfs:comment>
		<rdfs:comment xml:lang="OWLManchester">platform:comprisesInterfacePart some JavaSql</rdfs:comment>
	</owl:Class>
	<owl:Class rdf:about="&android-2_1;OrgXmlpullV1API">
		<owl:equivalentClass rdf:resource="&android-1_6;OrgXmlpullV1API"/>
		<rdfs:subClassOf rdf:resource="&java;JavaAPI"/>
		<rdfs:comment xml:lang="en">JavaLibrary implementing the org.xmlpull.v1 package for Android 2.1</rdfs:comment>
		<rdfs:comment xml:lang="OWLManchester">platform:comprisesInterfacePart some OrgXmlpullV1</rdfs:comment>
	</owl:Class>
	<owl:Class rdf:about="&android-2_1;OrgXmlpullV1Sax2API">
		<owl:equivalentClass rdf:resource="&android-1_6;OrgXmlpullV1Sax2API"/>
		<rdfs:subClassOf rdf:resource="&java;JavaAPI"/>
		<rdfs:comment xml:lang="en">JavaLibrary implementing the org.xmlpull.v1.sax2 package for Android 2.1</rdfs:comment>
		<rdfs:comment xml:lang="OWLManchester">platform:comprisesInterfacePart some OrgXmlpullV1Sax2</rdfs:comment>
	</owl:Class>
	<owl:Class rdf:about="&android-2_1;OrgXmlSaxAPI">
		<owl:equivalentClass rdf:resource="&java-se-6;OrgXmlSaxAPI"/>
		<owl:equivalentClass rdf:resource="&android-1_6;OrgXmlSaxAPI"/>
		<rdfs:subClassOf rdf:resource="&java;JavaAPI"/>
		<rdfs:comment xml:lang="en">JavaLibrary implementing the org.xml.sax package for Android 2.1</rdfs:comment>
		<rdfs:comment xml:lang="OWLManchester">platform:comprisesInterfacePart some OrgXmlSax</rdfs:comment>
	</owl:Class>
	<owl:Class rdf:about="&android-2_1;OrgXmlSaxHelpersAPI">
		<owl:equivalentClass rdf:resource="&java-se-6;OrgXmlSaxHelpersAPI"/>
		<owl:equivalentClass rdf:resource="&android-1_6;OrgXmlSaxHelpersAPI"/>
		<rdfs:subClassOf rdf:resource="&java;JavaAPI"/>
		<rdfs:comment xml:lang="en">JavaLibrary implementing the org.xml.sax.helpers package for Android 2.1</rdfs:comment>
		<rdfs:comment xml:lang="OWLManchester">platform:comprisesInterfacePart some OrgXmlSaxHelpers</rdfs:comment>
	</owl:Class>
	<owl:Class rdf:about="&android-2_1;OrgXmlSaxExtAPI">
		<owl:equivalentClass rdf:resource="&java-se-6;OrgXmlSaxExtAPI"/>
		<owl:equivalentClass rdf:resource="&android-1_6;OrgXmlSaxExtAPI"/>
		<rdfs:subClassOf rdf:resource="&java;JavaAPI"/>
		<rdfs:comment xml:lang="en">JavaLibrary implementing the org.xml.sax.ext package for Android 2.1</rdfs:comment>
		<rdfs:comment xml:lang="OWLManchester">platform:comprisesInterfacePart some OrgXmlSaxExt</rdfs:comment>
	</owl:Class>
	<owl:Class rdf:about="&android-2_1;OrgW3cDomAPI">
		<owl:equivalentClass rdf:resource="&android-1_6;OrgW3cDomAPI"/>
		<rdfs:subClassOf rdf:resource="&java;JavaAPI"/>
		<rdfs:comment xml:lang="en">JavaLibrary implementing the org.w3c.dom package for Android 2.1</rdfs:comment>
		<rdfs:comment xml:lang="OWLManchester">platform:comprisesInterfacePart some OrgW3cDom</rdfs:comment>
	</owl:Class>
	<owl:Class rdf:about="&android-2_1;OrgApacheCommonsLoggingAPI">
		<owl:equivalentClass rdf:resource="&android-1_6;OrgApacheCommonsLoggingAPI"/>
		<rdfs:subClassOf rdf:resource="&java;JavaAPI"/>
		<rdfs:comment xml:lang="en">JavaLibrary implementing the org.apache.commons.logging package for Android 2.1</rdfs:comment>
		<rdfs:comment xml:lang="OWLManchester">platform:comprisesInterfacePart some OrgApacheCommonsLogging</rdfs:comment>
	</owl:Class>
	<owl:Class rdf:about="&android-2_1;OrgApacheHttpAPI">
		<owl:equivalentClass rdf:resource="&android-1_6;OrgApacheHttpAPI"/>
		<rdfs:subClassOf rdf:resource="&java;JavaAPI"/>
		<rdfs:comment xml:lang="en">JavaLibrary implementing the org.apache.http package for Android 2.1</rdfs:comment>
		<rdfs:comment xml:lang="OWLManchester">platform:comprisesInterfacePart some OrgApacheHttp</rdfs:comment>
	</owl:Class>
	<owl:Class rdf:about="&android-2_1;OrgApacheHttpProtocolAPI">
		<owl:equivalentClass rdf:resource="&android-1_6;OrgApacheHttpProtocolAPI"/>
		<rdfs:subClassOf rdf:resource="&java;JavaAPI"/>
		<rdfs:comment xml:lang="en">JavaLibrary implementing the org.apache.http.protocol package for Android 2.1</rdfs:comment>
		<rdfs:comment xml:lang="OWLManchester">platform:comprisesInterfacePart some OrgApacheHttpProtocol</rdfs:comment>
	</owl:Class>
	<owl:Class rdf:about="&android-2_1;OrgApacheHttpUtilAPI">
		<owl:equivalentClass rdf:resource="&android-1_6;OrgApacheHttpUtilAPI"/>
		<rdfs:subClassOf rdf:resource="&java;JavaAPI"/>
		<rdfs:comment xml:lang="en">JavaLibrary implementing the org.apache.http.util package for Android 2.1</rdfs:comment>
		<rdfs:comment xml:lang="OWLManchester">platform:comprisesInterfacePart some OrgApacheHttpUtil</rdfs:comment>
	</owl:Class>
	<owl:Class rdf:about="&android-2_1;OrgApacheHttpParamsAPI">
		<owl:equivalentClass rdf:resource="&android-1_6;OrgApacheHttpParamsAPI"/>
		<rdfs:subClassOf rdf:resource="&java;JavaAPI"/>
		<rdfs:comment xml:lang="en">JavaLibrary implementing the org.apache.http.params package for Android 2.1</rdfs:comment>
		<rdfs:comment xml:lang="OWLManchester">platform:comprisesInterfacePart some OrgApacheHttpParams</rdfs:comment>
	</owl:Class>
	<owl:Class rdf:about="&android-2_1;OrgApacheHttpAuthAPI">
		<owl:equivalentClass rdf:resource="&android-1_6;OrgApacheHttpAuthAPI"/>
		<rdfs:subClassOf rdf:resource="&java;JavaAPI"/>
		<rdfs:comment xml:lang="en">JavaLibrary implementing the org.apache.http.auth package for Android 2.1</rdfs:comment>
		<rdfs:comment xml:lang="OWLManchester">platform:comprisesInterfacePart some OrgApacheHttpAuth</rdfs:comment>
	</owl:Class>
	<owl:Class rdf:about="&android-2_1;OrgApacheHttpAuthParamsAPI">
		<owl:equivalentClass rdf:resource="&android-1_6;OrgApacheHttpAuthParamsAPI"/>
		<rdfs:subClassOf rdf:resource="&java;JavaAPI"/>
		<rdfs:comment xml:lang="en">JavaLibrary implementing the org.apache.http.auth.params package for Android 2.1</rdfs:comment>
		<rdfs:comment xml:lang="OWLManchester">platform:comprisesInterfacePart some OrgApacheHttpAuthParams</rdfs:comment>
	</owl:Class>
	<owl:Class rdf:about="&android-2_1;OrgApacheHttpClientAPI">
		<owl:equivalentClass rdf:resource="&android-1_6;OrgApacheHttpClientAPI"/>
		<rdfs:subClassOf rdf:resource="&java;JavaAPI"/>
		<rdfs:comment xml:lang="en">JavaLibrary implementing the org.apache.http.client package for Android 2.1</rdfs:comment>
		<rdfs:comment xml:lang="OWLManchester">platform:comprisesInterfacePart some OrgApacheHttpClient</rdfs:comment>
	</owl:Class>
	<owl:Class rdf:about="&android-2_1;OrgApacheHttpClientMethodsAPI">
		<owl:equivalentClass rdf:resource="&android-1_6;OrgApacheHttpClientMethodsAPI"/>
		<rdfs:subClassOf rdf:resource="&java;JavaAPI"/>
		<rdfs:comment xml:lang="en">JavaLibrary implementing the org.apache.http.client.methods package for Android 2.1</rdfs:comment>
		<rdfs:comment xml:lang="OWLManchester">platform:comprisesInterfacePart some OrgApacheHttpClientMethods</rdfs:comment>
	</owl:Class>
	<owl:Class rdf:about="&android-2_1;OrgApacheHttpClientEntityAPI">
		<owl:equivalentClass rdf:resource="&android-1_6;OrgApacheHttpClientEntityAPI"/>
		<rdfs:subClassOf rdf:resource="&java;JavaAPI"/>
		<rdfs:comment xml:lang="en">JavaLibrary implementing the org.apache.http.client.entity package for Android 2.1</rdfs:comment>
		<rdfs:comment xml:lang="OWLManchester">platform:comprisesInterfacePart some OrgApacheHttpClientEntity</rdfs:comment>
	</owl:Class>
	<owl:Class rdf:about="&android-2_1;OrgApacheHttpClientParamsAPI">
		<owl:equivalentClass rdf:resource="&android-1_6;OrgApacheHttpClientParamsAPI"/>
		<rdfs:subClassOf rdf:resource="&java;JavaAPI"/>
		<rdfs:comment xml:lang="en">JavaLibrary implementing the org.apache.http.client.params package for Android 2.1</rdfs:comment>
		<rdfs:comment xml:lang="OWLManchester">platform:comprisesInterfacePart some OrgApacheHttpClientParams</rdfs:comment>
	</owl:Class>
	<owl:Class rdf:about="&android-2_1;OrgApacheHttpClientProtocolAPI">
		<owl:equivalentClass rdf:resource="&android-1_6;OrgApacheHttpClientProtocolAPI"/>
		<rdfs:subClassOf rdf:resource="&java;JavaAPI"/>
		<rdfs:comment xml:lang="en">JavaLibrary implementing the org.apache.http.client.protocol package for Android 2.1</rdfs:comment>
		<rdfs:comment xml:lang="OWLManchester">platform:comprisesInterfacePart some OrgApacheHttpClientProtocol</rdfs:comment>
	</owl:Class>
	<owl:Class rdf:about="&android-2_1;OrgApacheHttpClientUtilsAPI">
		<owl:equivalentClass rdf:resource="&android-1_6;OrgApacheHttpClientUtilsAPI"/>
		<rdfs:subClassOf rdf:resource="&java;JavaAPI"/>
		<rdfs:comment xml:lang="en">JavaLibrary implementing the org.apache.http.client.utils package for Android 2.1</rdfs:comment>
		<rdfs:comment xml:lang="OWLManchester">platform:comprisesInterfacePart some OrgApacheHttpClientUtils</rdfs:comment>
	</owl:Class>
	<owl:Class rdf:about="&android-2_1;OrgApacheHttpCookieAPI">
		<owl:equivalentClass rdf:resource="&android-1_6;OrgApacheHttpCookieAPI"/>
		<rdfs:subClassOf rdf:resource="&java;JavaAPI"/>
		<rdfs:comment xml:lang="en">JavaLibrary implementing the org.apache.http.cookie package for Android 2.1</rdfs:comment>
		<rdfs:comment xml:lang="OWLManchester">platform:comprisesInterfacePart some OrgApacheHttpCookie</rdfs:comment>
	</owl:Class>
	<owl:Class rdf:about="&android-2_1;OrgApacheHttpCookieParamsAPI">
		<owl:equivalentClass rdf:resource="&android-1_6;OrgApacheHttpCookieParamsAPI"/>
		<rdfs:subClassOf rdf:resource="&java;JavaAPI"/>
		<rdfs:comment xml:lang="en">JavaLibrary implementing the org.apache.http.cookie.params package for Android 2.1</rdfs:comment>
		<rdfs:comment xml:lang="OWLManchester">platform:comprisesInterfacePart some OrgApacheHttpCookieParams</rdfs:comment>
	</owl:Class>
	<owl:Class rdf:about="&android-2_1;OrgApacheHttpConnAPI">
		<owl:equivalentClass rdf:resource="&android-1_6;OrgApacheHttpConnAPI"/>
		<rdfs:subClassOf rdf:resource="&java;JavaAPI"/>
		<rdfs:comment xml:lang="en">JavaLibrary implementing the org.apache.http.conn package for Android 2.1</rdfs:comment>
		<rdfs:comment xml:lang="OWLManchester">platform:comprisesInterfacePart some OrgApacheHttpConn</rdfs:comment>
	</owl:Class>
	<owl:Class rdf:about="&android-2_1;OrgApacheHttpConnParamsAPI">
		<owl:equivalentClass rdf:resource="&android-1_6;OrgApacheHttpConnParamsAPI"/>
		<rdfs:subClassOf rdf:resource="&java;JavaAPI"/>
		<rdfs:comment xml:lang="en">JavaLibrary implementing the org.apache.http.conn.params package for Android 2.1</rdfs:comment>
		<rdfs:comment xml:lang="OWLManchester">platform:comprisesInterfacePart some OrgApacheHttpConnParams</rdfs:comment>
	</owl:Class>
	<owl:Class rdf:about="&android-2_1;OrgApacheHttpConnSchemeAPI">
		<owl:equivalentClass rdf:resource="&android-1_6;OrgApacheHttpConnSchemeAPI"/>
		<rdfs:subClassOf rdf:resource="&java;JavaAPI"/>
		<rdfs:comment xml:lang="en">JavaLibrary implementing the org.apache.http.conn.scheme package for Android 2.1</rdfs:comment>
		<rdfs:comment xml:lang="OWLManchester">platform:comprisesInterfacePart some OrgApacheHttpConnScheme</rdfs:comment>
	</owl:Class>
	<owl:Class rdf:about="&android-2_1;OrgApacheHttpConnRoutingAPI">
		<owl:equivalentClass rdf:resource="&android-1_6;OrgApacheHttpConnRoutingAPI"/>
		<rdfs:subClassOf rdf:resource="&java;JavaAPI"/>
		<rdfs:comment xml:lang="en">JavaLibrary implementing the org.apache.http.conn.routing package for Android 2.1</rdfs:comment>
		<rdfs:comment xml:lang="OWLManchester">platform:comprisesInterfacePart some OrgApacheHttpConnRouting</rdfs:comment>
	</owl:Class>
	<owl:Class rdf:about="&android-2_1;OrgApacheHttpConnSslAPI">
		<owl:equivalentClass rdf:resource="&android-1_6;OrgApacheHttpConnSslAPI"/>
		<rdfs:subClassOf rdf:resource="&java;JavaAPI"/>
		<rdfs:comment xml:lang="en">JavaLibrary implementing the org.apache.http.conn.ssl package for Android 2.1</rdfs:comment>
		<rdfs:comment xml:lang="OWLManchester">platform:comprisesInterfacePart some OrgApacheHttpConnSsl</rdfs:comment>
	</owl:Class>
	<owl:Class rdf:about="&android-2_1;OrgApacheHttpConnUtilAPI">
		<owl:equivalentClass rdf:resource="&android-1_6;OrgApacheHttpConnUtilAPI"/>
		<rdfs:subClassOf rdf:resource="&java;JavaAPI"/>
		<rdfs:comment xml:lang="en">JavaLibrary implementing the org.apache.http.conn.util package for Android 2.1</rdfs:comment>
		<rdfs:comment xml:lang="OWLManchester">platform:comprisesInterfacePart some OrgApacheHttpConnUtil</rdfs:comment>
	</owl:Class>
	<owl:Class rdf:about="&android-2_1;OrgApacheHttpEntityAPI">
		<owl:equivalentClass rdf:resource="&android-1_6;OrgApacheHttpEntityAPI"/>
		<rdfs:subClassOf rdf:resource="&java;JavaAPI"/>
		<rdfs:comment xml:lang="en">JavaLibrary implementing the org.apache.http.entity package for Android 2.1</rdfs:comment>
		<rdfs:comment xml:lang="OWLManchester">platform:comprisesInterfacePart some OrgApacheHttpEntity</rdfs:comment>
	</owl:Class>
	<owl:Class rdf:about="&android-2_1;OrgApacheHttpMessageAPI">
		<owl:equivalentClass rdf:resource="&android-1_6;OrgApacheHttpMessageAPI"/>
		<rdfs:subClassOf rdf:resource="&java;JavaAPI"/>
		<rdfs:comment xml:lang="en">JavaLibrary implementing the org.apache.http.message package for Android 2.1</rdfs:comment>
		<rdfs:comment xml:lang="OWLManchester">platform:comprisesInterfacePart some OrgApacheHttpMessage</rdfs:comment>
	</owl:Class>
	<owl:Class rdf:about="&android-2_1;OrgApacheHttpImplAPI">
		<owl:equivalentClass rdf:resource="&android-1_6;OrgApacheHttpImplAPI"/>
		<rdfs:subClassOf rdf:resource="&java;JavaAPI"/>
		<rdfs:comment xml:lang="en">JavaLibrary implementing the org.apache.http.impl package for Android 2.1</rdfs:comment>
		<rdfs:comment xml:lang="OWLManchester">platform:comprisesInterfacePart some OrgApacheHttpImpl</rdfs:comment>
	</owl:Class>
	<owl:Class rdf:about="&android-2_1;OrgApacheHttpImplEntityAPI">
		<owl:equivalentClass rdf:resource="&android-1_6;OrgApacheHttpImplEntityAPI"/>
		<rdfs:subClassOf rdf:resource="&java;JavaAPI"/>
		<rdfs:comment xml:lang="en">JavaLibrary implementing the org.apache.http.impl.entity package for Android 2.1</rdfs:comment>
		<rdfs:comment xml:lang="OWLManchester">platform:comprisesInterfacePart some OrgApacheHttpImplEntity</rdfs:comment>
	</owl:Class>
	<owl:Class rdf:about="&android-2_1;OrgApacheHttpImplAuthAPI">
		<owl:equivalentClass rdf:resource="&android-1_6;OrgApacheHttpImplAuthAPI"/>
		<rdfs:subClassOf rdf:resource="&java;JavaAPI"/>
		<rdfs:comment xml:lang="en">JavaLibrary implementing the org.apache.http.impl.auth package for Android 2.1</rdfs:comment>
		<rdfs:comment xml:lang="OWLManchester">platform:comprisesInterfacePart some OrgApacheHttpImplAuth</rdfs:comment>
	</owl:Class>
	<owl:Class rdf:about="&android-2_1;OrgApacheHttpImplClientAPI">
		<owl:equivalentClass rdf:resource="&android-1_6;OrgApacheHttpImplClientAPI"/>
		<rdfs:subClassOf rdf:resource="&java;JavaAPI"/>
		<rdfs:comment xml:lang="en">JavaLibrary implementing the org.apache.http.impl.client package for Android 2.1</rdfs:comment>
		<rdfs:comment xml:lang="OWLManchester">platform:comprisesInterfacePart some OrgApacheHttpImplClient</rdfs:comment>
	</owl:Class>
	<owl:Class rdf:about="&android-2_1;OrgApacheHttpImplConnAPI">
		<owl:equivalentClass rdf:resource="&android-1_6;OrgApacheHttpImplConnAPI"/>
		<rdfs:subClassOf rdf:resource="&java;JavaAPI"/>
		<rdfs:comment xml:lang="en">JavaLibrary implementing the org.apache.http.impl.conn package for Android 2.1</rdfs:comment>
		<rdfs:comment xml:lang="OWLManchester">platform:comprisesInterfacePart some OrgApacheHttpImplConn</rdfs:comment>
	</owl:Class>
	<owl:Class rdf:about="&android-2_1;OrgApacheHttpImplConnTsccmAPI">
		<owl:equivalentClass rdf:resource="&android-1_6;OrgApacheHttpImplConnTsccmAPI"/>
		<rdfs:subClassOf rdf:resource="&java;JavaAPI"/>
		<rdfs:comment xml:lang="en">JavaLibrary implementing the org.apache.http.impl.conn.tsccm package for Android 2.1</rdfs:comment>
		<rdfs:comment xml:lang="OWLManchester">platform:comprisesInterfacePart some OrgApacheHttpImplConnTsccm</rdfs:comment>
	</owl:Class>
	<owl:Class rdf:about="&android-2_1;OrgApacheHttpImplIoAPI">
		<owl:equivalentClass rdf:resource="&android-1_6;OrgApacheHttpImplIoAPI"/>
		<rdfs:subClassOf rdf:resource="&java;JavaAPI"/>
		<rdfs:comment xml:lang="en">JavaLibrary implementing the org.apache.http.impl.io package for Android 2.1</rdfs:comment>
		<rdfs:comment xml:lang="OWLManchester">platform:comprisesInterfacePart some OrgApacheHttpImplIo</rdfs:comment>
	</owl:Class>
	<owl:Class rdf:about="&android-2_1;OrgApacheHttpImplCookieAPI">
		<owl:equivalentClass rdf:resource="&android-1_6;OrgApacheHttpImplCookieAPI"/>
		<rdfs:subClassOf rdf:resource="&java;JavaAPI"/>
		<rdfs:comment xml:lang="en">JavaLibrary implementing the org.apache.http.impl.cookie package for Android 2.1</rdfs:comment>
		<rdfs:comment xml:lang="OWLManchester">platform:comprisesInterfacePart some OrgApacheHttpImplCookie</rdfs:comment>
	</owl:Class>
	<owl:Class rdf:about="&android-2_1;OrgApacheHttpIoAPI">
		<owl:equivalentClass rdf:resource="&android-1_6;OrgApacheHttpIoAPI"/>
		<rdfs:subClassOf rdf:resource="&java;JavaAPI"/>
		<rdfs:comment xml:lang="en">JavaLibrary implementing the org.apache.http.io package for Android 2.1</rdfs:comment>
		<rdfs:comment xml:lang="OWLManchester">platform:comprisesInterfacePart some OrgApacheHttpIo</rdfs:comment>
	</owl:Class>
	<owl:Class rdf:about="&android-2_1;OrgJsonAPI">
		<owl:equivalentClass rdf:resource="&android-1_6;OrgJsonAPI"/>
		<rdfs:subClassOf rdf:resource="&java;JavaAPI"/>
		<rdfs:comment xml:lang="en">JavaLibrary implementing the org.json package for Android 2.1</rdfs:comment>
		<rdfs:comment xml:lang="OWLManchester">platform:comprisesInterfacePart some OrgJson</rdfs:comment>
	</owl:Class>
	<owl:Class rdf:about="&android-2_1;JavaxMicroeditionKhronosOpenglesAPI">
		<owl:equivalentClass rdf:resource="&android-1_6;JavaxMicroeditionKhronosOpenglesAPI"/>
		<rdfs:subClassOf rdf:resource="&java;JavaAPI"/>
		<rdfs:comment xml:lang="en">JavaLibrary implementing the javax.microedition.khronos.opengles package for Android 2.1</rdfs:comment>
		<rdfs:comment xml:lang="OWLManchester">platform:comprisesInterfacePart some JavaxMicroeditionKhronosOpengles</rdfs:comment>
	</owl:Class>
	<owl:Class rdf:about="&android-2_1;JavaxMicroeditionKhronosEglAPI">
		<owl:equivalentClass rdf:resource="&android-1_6;JavaxMicroeditionKhronosEglAPI"/>
		<rdfs:subClassOf rdf:resource="&java;JavaAPI"/>
		<rdfs:comment xml:lang="en">JavaLibrary implementing the javax.microedition.khronos.egl package for Android 2.1</rdfs:comment>
		<rdfs:comment xml:lang="OWLManchester">platform:comprisesInterfacePart some JavaxMicroeditionKhronosEgl</rdfs:comment>
	</owl:Class>
	<owl:Class rdf:about="&android-2_1;JavaxNetAPI">
		<owl:equivalentClass rdf:resource="&java-se-6;JavaxNetAPI"/>
		<owl:equivalentClass rdf:resource="&android-1_6;JavaxNetAPI"/>
		<rdfs:subClassOf rdf:resource="&java;JavaAPI"/>
		<rdfs:comment xml:lang="en">JavaLibrary implementing the javax.net package for Android 2.1</rdfs:comment>
		<rdfs:comment xml:lang="OWLManchester">platform:comprisesInterfacePart some JavaxNet</rdfs:comment>
	</owl:Class>
	<owl:Class rdf:about="&android-2_1;JavaxNetSslAPI">
		<owl:equivalentClass rdf:resource="&android-1_6;JavaxNetSslAPI"/>
		<rdfs:subClassOf rdf:resource="&java;JavaAPI"/>
		<rdfs:comment xml:lang="en">JavaLibrary implementing the javax.net.ssl package for Android 2.1</rdfs:comment>
		<rdfs:comment xml:lang="OWLManchester">platform:comprisesInterfacePart some JavaxNetSsl</rdfs:comment>
	</owl:Class>
	<owl:Class rdf:about="&android-2_1;JavaxSecurityAuthAPI">
		<owl:equivalentClass rdf:resource="&android-1_6;JavaxSecurityAuthAPI"/>
		<rdfs:subClassOf rdf:resource="&java;JavaAPI"/>
		<rdfs:comment xml:lang="en">JavaLibrary implementing the javax.security.auth package for Android 2.1</rdfs:comment>
		<rdfs:comment xml:lang="OWLManchester">platform:comprisesInterfacePart some JavaxSecurityAuth</rdfs:comment>
	</owl:Class>
	<owl:Class rdf:about="&android-2_1;JavaxSecurityAuthCallbackAPI">
		<owl:equivalentClass rdf:resource="&android-1_6;JavaxSecurityAuthCallbackAPI"/>
		<rdfs:subClassOf rdf:resource="&java;JavaAPI"/>
		<rdfs:comment xml:lang="en">JavaLibrary implementing the javax.security.auth.callback package for Android 2.1</rdfs:comment>
		<rdfs:comment xml:lang="OWLManchester">platform:comprisesInterfacePart some JavaxSecurityAuthCallback</rdfs:comment>
	</owl:Class>
	<owl:Class rdf:about="&android-2_1;JavaxSecurityAuthX500API">
		<owl:equivalentClass rdf:resource="&android-1_6;JavaxSecurityAuthX500API"/>
		<rdfs:subClassOf rdf:resource="&java;JavaAPI"/>
		<rdfs:comment xml:lang="en">JavaLibrary implementing the javax.security.auth.x500 package for Android 2.1</rdfs:comment>
		<rdfs:comment xml:lang="OWLManchester">platform:comprisesInterfacePart some JavaxSecurityAuthX500</rdfs:comment>
	</owl:Class>
	<owl:Class rdf:about="&android-2_1;JavaxSecurityAuthLoginAPI">
		<owl:equivalentClass rdf:resource="&android-1_6;JavaxSecurityAuthLoginAPI"/>
		<rdfs:subClassOf rdf:resource="&java;JavaAPI"/>
		<rdfs:comment xml:lang="en">JavaLibrary implementing the javax.security.auth.login package for Android 2.1</rdfs:comment>
		<rdfs:comment xml:lang="OWLManchester">platform:comprisesInterfacePart some JavaxSecurityAuthLogin</rdfs:comment>
	</owl:Class>
	<owl:Class rdf:about="&android-2_1;JavaxSecurityCertAPI">
		<owl:equivalentClass rdf:resource="&java-se-6;JavaxSecurityCertAPI"/>
		<owl:equivalentClass rdf:resource="&android-1_6;JavaxSecurityCertAPI"/>
		<rdfs:subClassOf rdf:resource="&java;JavaAPI"/>
		<rdfs:comment xml:lang="en">JavaLibrary implementing the javax.security.cert package for Android 2.1</rdfs:comment>
		<rdfs:comment xml:lang="OWLManchester">platform:comprisesInterfacePart some JavaxSecurityCert</rdfs:comment>
	</owl:Class>
	<owl:Class rdf:about="&android-2_1;JavaxCryptoAPI">
		<owl:equivalentClass rdf:resource="&java-se-6;JavaxCryptoAPI"/>
		<owl:equivalentClass rdf:resource="&android-1_6;JavaxCryptoAPI"/>
		<rdfs:subClassOf rdf:resource="&java;JavaAPI"/>
		<rdfs:comment xml:lang="en">JavaLibrary implementing the javax.crypto package for Android 2.1</rdfs:comment>
		<rdfs:comment xml:lang="OWLManchester">platform:comprisesInterfacePart some JavaxCrypto</rdfs:comment>
	</owl:Class>
	<owl:Class rdf:about="&android-2_1;JavaxCryptoInterfacesAPI">
		<owl:equivalentClass rdf:resource="&java-se-6;JavaxCryptoInterfacesAPI"/>
		<owl:equivalentClass rdf:resource="&android-1_6;JavaxCryptoInterfacesAPI"/>
		<rdfs:subClassOf rdf:resource="&java;JavaAPI"/>
		<rdfs:comment xml:lang="en">JavaLibrary implementing the javax.crypto.interfaces package for Android 2.1</rdfs:comment>
		<rdfs:comment xml:lang="OWLManchester">platform:comprisesInterfacePart some JavaxCryptoInterfaces</rdfs:comment>
	</owl:Class>
	<owl:Class rdf:about="&android-2_1;JavaxCryptoSpecAPI">
		<owl:equivalentClass rdf:resource="&java-se-6;JavaxCryptoSpecAPI"/>
		<owl:equivalentClass rdf:resource="&android-1_6;JavaxCryptoSpecAPI"/>
		<rdfs:subClassOf rdf:resource="&java;JavaAPI"/>
		<rdfs:comment xml:lang="en">JavaLibrary implementing the javax.crypto.spec package for Android 2.1</rdfs:comment>
		<rdfs:comment xml:lang="OWLManchester">platform:comprisesInterfacePart some JavaxCryptoSpec</rdfs:comment>
	</owl:Class>
	<owl:Class rdf:about="&android-2_1;JavaxSqlAPI">
		<owl:equivalentClass rdf:resource="&android-1_6;JavaxSqlAPI"/>
		<rdfs:subClassOf rdf:resource="&java;JavaAPI"/>
		<rdfs:comment xml:lang="en">JavaLibrary implementing the javax.sql package for Android 2.1</rdfs:comment>
		<rdfs:comment xml:lang="OWLManchester">platform:comprisesInterfacePart some JavaxSql</rdfs:comment>
	</owl:Class>
	<owl:Class rdf:about="&android-2_1;JavaxXmlAPI">
		<owl:equivalentClass rdf:resource="&android-1_6;JavaxXmlAPI"/>
		<rdfs:subClassOf rdf:resource="&java-se-6;JavaxXmlAPI"/>
		<rdfs:comment xml:lang="en">JavaLibrary implementing the javax.xml package for Android 2.1</rdfs:comment>
		<rdfs:comment xml:lang="OWLManchester">platform:comprisesInterfacePart some JavaxXml</rdfs:comment>
	</owl:Class>
	<owl:Class rdf:about="&android-2_1;JavaxXmlParsersAPI">
		<owl:equivalentClass rdf:resource="&android-1_6;JavaxXmlParsersAPI"/>
		<rdfs:subClassOf rdf:resource="&java;JavaAPI"/>
		<rdfs:comment xml:lang="en">JavaLibrary implementing the javax.xml.parsers package for Android 2.1</rdfs:comment>
		<rdfs:comment xml:lang="OWLManchester">platform:comprisesInterfacePart some JavaxXmlParsers</rdfs:comment>
	</owl:Class>
	<owl:Class rdf:about="&android-2_1;JunitFrameworkAPI">
		<owl:equivalentClass rdf:resource="&android-1_6;JunitFrameworkAPI"/>
		<rdfs:subClassOf rdf:resource="&java;JavaAPI"/>
		<rdfs:comment xml:lang="en">JavaLibrary implementing the junit.framework package for Android 2.1</rdfs:comment>
		<rdfs:comment xml:lang="OWLManchester">platform:comprisesInterfacePart some JunitFramework</rdfs:comment>
	</owl:Class>
	<owl:Class rdf:about="&android-2_1;JunitRunnerAPI">
		<owl:equivalentClass rdf:resource="&android-1_6;JunitRunnerAPI"/>
		<rdfs:subClassOf rdf:resource="&java;JavaAPI"/>
		<rdfs:comment xml:lang="en">JavaLibrary implementing the junit.runner package for Android 2.1</rdfs:comment>
		<rdfs:comment xml:lang="OWLManchester">platform:comprisesInterfacePart some JunitRunner</rdfs:comment>
	</owl:Class>
	<owl:Class rdf:about="&android-2_1;DalvikAnnotationAPI">
		<owl:equivalentClass rdf:resource="&android-1_6;DalvikAnnotationAPI"/>
		<rdfs:subClassOf rdf:resource="&java;JavaAPI"/>
		<rdfs:comment xml:lang="en">JavaLibrary implementing the dalvik.annotation package for Android 2.1</rdfs:comment>
		<rdfs:comment xml:lang="OWLManchester">platform:comprisesInterfacePart some DalvikAnnotation</rdfs:comment>
	</owl:Class>
	<owl:Class rdf:about="&android-2_1;DalvikBytecodeAPI">
		<owl:equivalentClass rdf:resource="&android-1_6;DalvikBytecodeAPI"/>
		<rdfs:subClassOf rdf:resource="&java;JavaAPI"/>
		<rdfs:comment xml:lang="en">JavaLibrary implementing the dalvik.bytecode package for Android 2.1</rdfs:comment>
		<rdfs:comment xml:lang="OWLManchester">platform:comprisesInterfacePart some DalvikBytecode</rdfs:comment>
	</owl:Class>
	<owl:Class rdf:about="&android-2_1;DalvikSystemAPI">
		<owl:equivalentClass rdf:resource="&android-1_6;DalvikSystemAPI"/>
		<rdfs:subClassOf rdf:resource="&java;JavaAPI"/>
		<rdfs:comment xml:lang="en">JavaLibrary implementing the dalvik.system package for Android 2.1</rdfs:comment>
		<rdfs:comment xml:lang="OWLManchester">platform:comprisesInterfacePart some DalvikSystem</rdfs:comment>
	</owl:Class>
	<android-2_1:Android rdf:about="&android-2_1;theAndroidPart">
	</android-2_1:Android>
	<android-2_1:AndroidAccessibilityservice rdf:about="&android-2_1;theAndroidAccessibilityservicePart">
	</android-2_1:AndroidAccessibilityservice>
	<android-2_1:AndroidApp rdf:about="&android-2_1;theAndroidAppPart">
	</android-2_1:AndroidApp>
	<android-2_1:AndroidView rdf:about="&android-2_1;theAndroidViewPart">
	</android-2_1:AndroidView>
	<android-2_1:AndroidViewAccessibility rdf:about="&android-2_1;theAndroidViewAccessibilityPart">
	</android-2_1:AndroidViewAccessibility>
	<android-2_1:AndroidViewInputmethod rdf:about="&android-2_1;theAndroidViewInputmethodPart">
	</android-2_1:AndroidViewInputmethod>
	<android-2_1:AndroidViewAnimation rdf:about="&android-2_1;theAndroidViewAnimationPart">
	</android-2_1:AndroidViewAnimation>
	<android-2_1:AndroidContent rdf:about="&android-2_1;theAndroidContentPart">
	</android-2_1:AndroidContent>
	<android-2_1:AndroidContentRes rdf:about="&android-2_1;theAndroidContentResPart">
	</android-2_1:AndroidContentRes>
	<android-2_1:AndroidContentPm rdf:about="&android-2_1;theAndroidContentPmPart">
	</android-2_1:AndroidContentPm>
	<android-2_1:AndroidOs rdf:about="&android-2_1;theAndroidOsPart">
	</android-2_1:AndroidOs>
	<android-2_1:AndroidAccounts rdf:about="&android-2_1;theAndroidAccountsPart">
	</android-2_1:AndroidAccounts>
	<android-2_1:AndroidGraphics rdf:about="&android-2_1;theAndroidGraphicsPart">
	</android-2_1:AndroidGraphics>
	<android-2_1:AndroidGraphicsDrawable rdf:about="&android-2_1;theAndroidGraphicsDrawablePart">
	</android-2_1:AndroidGraphicsDrawable>
	<android-2_1:AndroidGraphicsDrawableShapes rdf:about="&android-2_1;theAndroidGraphicsDrawableShapesPart">
	</android-2_1:AndroidGraphicsDrawableShapes>
	<android-2_1:AndroidNet rdf:about="&android-2_1;theAndroidNetPart">
	</android-2_1:AndroidNet>
	<android-2_1:AndroidNetHttp rdf:about="&android-2_1;theAndroidNetHttpPart">
	</android-2_1:AndroidNetHttp>
	<android-2_1:AndroidNetWifi rdf:about="&android-2_1;theAndroidNetWifiPart">
	</android-2_1:AndroidNetWifi>
	<android-2_1:AndroidDatabase rdf:about="&android-2_1;theAndroidDatabasePart">
	</android-2_1:AndroidDatabase>
	<android-2_1:AndroidDatabaseSqlite rdf:about="&android-2_1;theAndroidDatabaseSqlitePart">
	</android-2_1:AndroidDatabaseSqlite>
	<android-2_1:AndroidUtil rdf:about="&android-2_1;theAndroidUtilPart">
	</android-2_1:AndroidUtil>
	<android-2_1:AndroidWidget rdf:about="&android-2_1;theAndroidWidgetPart">
	</android-2_1:AndroidWidget>
	<android-2_1:AndroidAppwidget rdf:about="&android-2_1;theAndroidAppwidgetPart">
	</android-2_1:AndroidAppwidget>
	<android-2_1:AndroidBluetooth rdf:about="&android-2_1;theAndroidBluetoothPart">
	</android-2_1:AndroidBluetooth>
	<android-2_1:AndroidGesture rdf:about="&android-2_1;theAndroidGesturePart">
	</android-2_1:AndroidGesture>
	<android-2_1:AndroidHardware rdf:about="&android-2_1;theAndroidHardwarePart">
	</android-2_1:AndroidHardware>
	<android-2_1:AndroidInputmethodservice rdf:about="&android-2_1;theAndroidInputmethodservicePart">
	</android-2_1:AndroidInputmethodservice>
	<android-2_1:AndroidLocation rdf:about="&android-2_1;theAndroidLocationPart">
	</android-2_1:AndroidLocation>
	<android-2_1:AndroidMedia rdf:about="&android-2_1;theAndroidMediaPart">
	</android-2_1:AndroidMedia>
	<android-2_1:AndroidOpengl rdf:about="&android-2_1;theAndroidOpenglPart">
	</android-2_1:AndroidOpengl>
	<android-2_1:AndroidPreference rdf:about="&android-2_1;theAndroidPreferencePart">
	</android-2_1:AndroidPreference>
	<android-2_1:AndroidProvider rdf:about="&android-2_1;theAndroidProviderPart">
	</android-2_1:AndroidProvider>
	<android-2_1:AndroidWebkit rdf:about="&android-2_1;theAndroidWebkitPart">
	</android-2_1:AndroidWebkit>
	<android-2_1:AndroidSax rdf:about="&android-2_1;theAndroidSaxPart">
	</android-2_1:AndroidSax>
	<android-2_1:AndroidServiceWallpaper rdf:about="&android-2_1;theAndroidServiceWallpaperPart">
	</android-2_1:AndroidServiceWallpaper>
	<android-2_1:AndroidSpeech rdf:about="&android-2_1;theAndroidSpeechPart">
	</android-2_1:AndroidSpeech>
	<android-2_1:AndroidSpeechTts rdf:about="&android-2_1;theAndroidSpeechTtsPart">
	</android-2_1:AndroidSpeechTts>
	<android-2_1:AndroidTelephony rdf:about="&android-2_1;theAndroidTelephonyPart">
	</android-2_1:AndroidTelephony>
	<android-2_1:AndroidTelephonyCdma rdf:about="&android-2_1;theAndroidTelephonyCdmaPart">
	</android-2_1:AndroidTelephonyCdma>
	<android-2_1:AndroidTelephonyGsm rdf:about="&android-2_1;theAndroidTelephonyGsmPart">
	</android-2_1:AndroidTelephonyGsm>
	<android-2_1:AndroidText rdf:about="&android-2_1;theAndroidTextPart">
	</android-2_1:AndroidText>
	<android-2_1:AndroidTextFormat rdf:about="&android-2_1;theAndroidTextFormatPart">
	</android-2_1:AndroidTextFormat>
	<android-2_1:AndroidTextMethod rdf:about="&android-2_1;theAndroidTextMethodPart">
	</android-2_1:AndroidTextMethod>
	<android-2_1:AndroidTextStyle rdf:about="&android-2_1;theAndroidTextStylePart">
	</android-2_1:AndroidTextStyle>
	<android-2_1:AndroidTextUtil rdf:about="&android-2_1;theAndroidTextUtilPart">
	</android-2_1:AndroidTextUtil>
	<android-2_1:AndroidTest rdf:about="&android-2_1;theAndroidTestPart">
	</android-2_1:AndroidTest>
	<android-2_1:AndroidTestMock rdf:about="&android-2_1;theAndroidTestMockPart">
	</android-2_1:AndroidTestMock>
	<android-2_1:AndroidTestSuitebuilder rdf:about="&android-2_1;theAndroidTestSuitebuilderPart">
	</android-2_1:AndroidTestSuitebuilder>
	<android-2_1:AndroidTestSuitebuilderAnnotation rdf:about="&android-2_1;theAndroidTestSuitebuilderAnnotationPart">
	</android-2_1:AndroidTestSuitebuilderAnnotation>
	<android-2_1:JavaLang rdf:about="&android-2_1;theJavaLangPart">
	</android-2_1:JavaLang>
	<android-2_1:JavaLangAnnotation rdf:about="&android-2_1;theJavaLangAnnotationPart">
	</android-2_1:JavaLangAnnotation>
	<android-2_1:JavaLangReflect rdf:about="&android-2_1;theJavaLangReflectPart">
	</android-2_1:JavaLangReflect>
	<android-2_1:JavaLangRef rdf:about="&android-2_1;theJavaLangRefPart">
	</android-2_1:JavaLangRef>
	<android-2_1:JavaUtil rdf:about="&android-2_1;theJavaUtilPart">
	</android-2_1:JavaUtil>
	<android-2_1:JavaUtilConcurrent rdf:about="&android-2_1;theJavaUtilConcurrentPart">
	</android-2_1:JavaUtilConcurrent>
	<android-2_1:JavaUtilConcurrentAtomic rdf:about="&android-2_1;theJavaUtilConcurrentAtomicPart">
	</android-2_1:JavaUtilConcurrentAtomic>
	<android-2_1:JavaUtilConcurrentLocks rdf:about="&android-2_1;theJavaUtilConcurrentLocksPart">
	</android-2_1:JavaUtilConcurrentLocks>
	<android-2_1:JavaUtilRegex rdf:about="&android-2_1;theJavaUtilRegexPart">
	</android-2_1:JavaUtilRegex>
	<android-2_1:JavaUtilJar rdf:about="&android-2_1;theJavaUtilJarPart">
	</android-2_1:JavaUtilJar>
	<android-2_1:JavaUtilZip rdf:about="&android-2_1;theJavaUtilZipPart">
	</android-2_1:JavaUtilZip>
	<android-2_1:JavaUtilLogging rdf:about="&android-2_1;theJavaUtilLoggingPart">
	</android-2_1:JavaUtilLogging>
	<android-2_1:JavaUtilPrefs rdf:about="&android-2_1;theJavaUtilPrefsPart">
	</android-2_1:JavaUtilPrefs>
	<android-2_1:JavaIo rdf:about="&android-2_1;theJavaIoPart">
	</android-2_1:JavaIo>
	<android-2_1:JavaNio rdf:about="&android-2_1;theJavaNioPart">
	</android-2_1:JavaNio>
	<android-2_1:JavaNioChannels rdf:about="&android-2_1;theJavaNioChannelsPart">
	</android-2_1:JavaNioChannels>
	<android-2_1:JavaNioChannelsSpi rdf:about="&android-2_1;theJavaNioChannelsSpiPart">
	</android-2_1:JavaNioChannelsSpi>
	<android-2_1:JavaNioCharset rdf:about="&android-2_1;theJavaNioCharsetPart">
	</android-2_1:JavaNioCharset>
	<android-2_1:JavaNioCharsetSpi rdf:about="&android-2_1;theJavaNioCharsetSpiPart">
	</android-2_1:JavaNioCharsetSpi>
	<android-2_1:JavaNet rdf:about="&android-2_1;theJavaNetPart">
	</android-2_1:JavaNet>
	<android-2_1:JavaSecurity rdf:about="&android-2_1;theJavaSecurityPart">
	</android-2_1:JavaSecurity>
	<android-2_1:JavaSecurityCert rdf:about="&android-2_1;theJavaSecurityCertPart">
	</android-2_1:JavaSecurityCert>
	<android-2_1:JavaSecuritySpec rdf:about="&android-2_1;theJavaSecuritySpecPart">
	</android-2_1:JavaSecuritySpec>
	<android-2_1:JavaSecurityAcl rdf:about="&android-2_1;theJavaSecurityAclPart">
	</android-2_1:JavaSecurityAcl>
	<android-2_1:JavaSecurityInterfaces rdf:about="&android-2_1;theJavaSecurityInterfacesPart">
	</android-2_1:JavaSecurityInterfaces>
	<android-2_1:JavaText rdf:about="&android-2_1;theJavaTextPart">
	</android-2_1:JavaText>
	<android-2_1:JavaAwtFont rdf:about="&android-2_1;theJavaAwtFontPart">
	</android-2_1:JavaAwtFont>
	<android-2_1:JavaBeans rdf:about="&android-2_1;theJavaBeansPart">
	</android-2_1:JavaBeans>
	<android-2_1:JavaMath rdf:about="&android-2_1;theJavaMathPart">
	</android-2_1:JavaMath>
	<android-2_1:JavaSql rdf:about="&android-2_1;theJavaSqlPart">
	</android-2_1:JavaSql>
	<android-2_1:OrgXmlpullV1 rdf:about="&android-2_1;theOrgXmlpullV1Part">
	</android-2_1:OrgXmlpullV1>
	<android-2_1:OrgXmlpullV1Sax2 rdf:about="&android-2_1;theOrgXmlpullV1Sax2Part">
	</android-2_1:OrgXmlpullV1Sax2>
	<android-2_1:OrgXmlSax rdf:about="&android-2_1;theOrgXmlSaxPart">
	</android-2_1:OrgXmlSax>
	<android-2_1:OrgXmlSaxHelpers rdf:about="&android-2_1;theOrgXmlSaxHelpersPart">
	</android-2_1:OrgXmlSaxHelpers>
	<android-2_1:OrgXmlSaxExt rdf:about="&android-2_1;theOrgXmlSaxExtPart">
	</android-2_1:OrgXmlSaxExt>
	<android-2_1:OrgW3cDom rdf:about="&android-2_1;theOrgW3cDomPart">
	</android-2_1:OrgW3cDom>
	<android-2_1:OrgApacheCommonsLogging rdf:about="&android-2_1;theOrgApacheCommonsLoggingPart">
	</android-2_1:OrgApacheCommonsLogging>
	<android-2_1:OrgApacheHttp rdf:about="&android-2_1;theOrgApacheHttpPart">
	</android-2_1:OrgApacheHttp>
	<android-2_1:OrgApacheHttpProtocol rdf:about="&android-2_1;theOrgApacheHttpProtocolPart">
	</android-2_1:OrgApacheHttpProtocol>
	<android-2_1:OrgApacheHttpUtil rdf:about="&android-2_1;theOrgApacheHttpUtilPart">
	</android-2_1:OrgApacheHttpUtil>
	<android-2_1:OrgApacheHttpParams rdf:about="&android-2_1;theOrgApacheHttpParamsPart">
	</android-2_1:OrgApacheHttpParams>
	<android-2_1:OrgApacheHttpAuth rdf:about="&android-2_1;theOrgApacheHttpAuthPart">
	</android-2_1:OrgApacheHttpAuth>
	<android-2_1:OrgApacheHttpAuthParams rdf:about="&android-2_1;theOrgApacheHttpAuthParamsPart">
	</android-2_1:OrgApacheHttpAuthParams>
	<android-2_1:OrgApacheHttpClient rdf:about="&android-2_1;theOrgApacheHttpClientPart">
	</android-2_1:OrgApacheHttpClient>
	<android-2_1:OrgApacheHttpClientMethods rdf:about="&android-2_1;theOrgApacheHttpClientMethodsPart">
	</android-2_1:OrgApacheHttpClientMethods>
	<android-2_1:OrgApacheHttpClientEntity rdf:about="&android-2_1;theOrgApacheHttpClientEntityPart">
	</android-2_1:OrgApacheHttpClientEntity>
	<android-2_1:OrgApacheHttpClientParams rdf:about="&android-2_1;theOrgApacheHttpClientParamsPart">
	</android-2_1:OrgApacheHttpClientParams>
	<android-2_1:OrgApacheHttpClientProtocol rdf:about="&android-2_1;theOrgApacheHttpClientProtocolPart">
	</android-2_1:OrgApacheHttpClientProtocol>
	<android-2_1:OrgApacheHttpClientUtils rdf:about="&android-2_1;theOrgApacheHttpClientUtilsPart">
	</android-2_1:OrgApacheHttpClientUtils>
	<android-2_1:OrgApacheHttpCookie rdf:about="&android-2_1;theOrgApacheHttpCookiePart">
	</android-2_1:OrgApacheHttpCookie>
	<android-2_1:OrgApacheHttpCookieParams rdf:about="&android-2_1;theOrgApacheHttpCookieParamsPart">
	</android-2_1:OrgApacheHttpCookieParams>
	<android-2_1:OrgApacheHttpConn rdf:about="&android-2_1;theOrgApacheHttpConnPart">
	</android-2_1:OrgApacheHttpConn>
	<android-2_1:OrgApacheHttpConnParams rdf:about="&android-2_1;theOrgApacheHttpConnParamsPart">
	</android-2_1:OrgApacheHttpConnParams>
	<android-2_1:OrgApacheHttpConnScheme rdf:about="&android-2_1;theOrgApacheHttpConnSchemePart">
	</android-2_1:OrgApacheHttpConnScheme>
	<android-2_1:OrgApacheHttpConnRouting rdf:about="&android-2_1;theOrgApacheHttpConnRoutingPart">
	</android-2_1:OrgApacheHttpConnRouting>
	<android-2_1:OrgApacheHttpConnSsl rdf:about="&android-2_1;theOrgApacheHttpConnSslPart">
	</android-2_1:OrgApacheHttpConnSsl>
	<android-2_1:OrgApacheHttpConnUtil rdf:about="&android-2_1;theOrgApacheHttpConnUtilPart">
	</android-2_1:OrgApacheHttpConnUtil>
	<android-2_1:OrgApacheHttpEntity rdf:about="&android-2_1;theOrgApacheHttpEntityPart">
	</android-2_1:OrgApacheHttpEntity>
	<android-2_1:OrgApacheHttpMessage rdf:about="&android-2_1;theOrgApacheHttpMessagePart">
	</android-2_1:OrgApacheHttpMessage>
	<android-2_1:OrgApacheHttpImpl rdf:about="&android-2_1;theOrgApacheHttpImplPart">
	</android-2_1:OrgApacheHttpImpl>
	<android-2_1:OrgApacheHttpImplEntity rdf:about="&android-2_1;theOrgApacheHttpImplEntityPart">
	</android-2_1:OrgApacheHttpImplEntity>
	<android-2_1:OrgApacheHttpImplAuth rdf:about="&android-2_1;theOrgApacheHttpImplAuthPart">
	</android-2_1:OrgApacheHttpImplAuth>
	<android-2_1:OrgApacheHttpImplClient rdf:about="&android-2_1;theOrgApacheHttpImplClientPart">
	</android-2_1:OrgApacheHttpImplClient>
	<android-2_1:OrgApacheHttpImplConn rdf:about="&android-2_1;theOrgApacheHttpImplConnPart">
	</android-2_1:OrgApacheHttpImplConn>
	<android-2_1:OrgApacheHttpImplConnTsccm rdf:about="&android-2_1;theOrgApacheHttpImplConnTsccmPart">
	</android-2_1:OrgApacheHttpImplConnTsccm>
	<android-2_1:OrgApacheHttpImplIo rdf:about="&android-2_1;theOrgApacheHttpImplIoPart">
	</android-2_1:OrgApacheHttpImplIo>
	<android-2_1:OrgApacheHttpImplCookie rdf:about="&android-2_1;theOrgApacheHttpImplCookiePart">
	</android-2_1:OrgApacheHttpImplCookie>
	<android-2_1:OrgApacheHttpIo rdf:about="&android-2_1;theOrgApacheHttpIoPart">
	</android-2_1:OrgApacheHttpIo>
	<android-2_1:OrgJson rdf:about="&android-2_1;theOrgJsonPart">
	</android-2_1:OrgJson>
	<android-2_1:JavaxMicroeditionKhronosOpengles rdf:about="&android-2_1;theJavaxMicroeditionKhronosOpenglesPart">
	</android-2_1:JavaxMicroeditionKhronosOpengles>
	<android-2_1:JavaxMicroeditionKhronosEgl rdf:about="&android-2_1;theJavaxMicroeditionKhronosEglPart">
	</android-2_1:JavaxMicroeditionKhronosEgl>
	<android-2_1:JavaxNet rdf:about="&android-2_1;theJavaxNetPart">
	</android-2_1:JavaxNet>
	<android-2_1:JavaxNetSsl rdf:about="&android-2_1;theJavaxNetSslPart">
	</android-2_1:JavaxNetSsl>
	<android-2_1:JavaxSecurityAuth rdf:about="&android-2_1;theJavaxSecurityAuthPart">
	</android-2_1:JavaxSecurityAuth>
	<android-2_1:JavaxSecurityAuthCallback rdf:about="&android-2_1;theJavaxSecurityAuthCallbackPart">
	</android-2_1:JavaxSecurityAuthCallback>
	<android-2_1:JavaxSecurityAuthX500 rdf:about="&android-2_1;theJavaxSecurityAuthX500Part">
	</android-2_1:JavaxSecurityAuthX500>
	<android-2_1:JavaxSecurityAuthLogin rdf:about="&android-2_1;theJavaxSecurityAuthLoginPart">
	</android-2_1:JavaxSecurityAuthLogin>
	<android-2_1:JavaxSecurityCert rdf:about="&android-2_1;theJavaxSecurityCertPart">
	</android-2_1:JavaxSecurityCert>
	<android-2_1:JavaxCrypto rdf:about="&android-2_1;theJavaxCryptoPart">
	</android-2_1:JavaxCrypto>
	<android-2_1:JavaxCryptoInterfaces rdf:about="&android-2_1;theJavaxCryptoInterfacesPart">
	</android-2_1:JavaxCryptoInterfaces>
	<android-2_1:JavaxCryptoSpec rdf:about="&android-2_1;theJavaxCryptoSpecPart">
	</android-2_1:JavaxCryptoSpec>
	<android-2_1:JavaxSql rdf:about="&android-2_1;theJavaxSqlPart">
	</android-2_1:JavaxSql>
	<android-2_1:JavaxXml rdf:about="&android-2_1;theJavaxXmlPart">
	</android-2_1:JavaxXml>
	<android-2_1:JavaxXmlParsers rdf:about="&android-2_1;theJavaxXmlParsersPart">
	</android-2_1:JavaxXmlParsers>
	<android-2_1:JunitFramework rdf:about="&android-2_1;theJunitFrameworkPart">
	</android-2_1:JunitFramework>
	<android-2_1:JunitRunner rdf:about="&android-2_1;theJunitRunnerPart">
	</android-2_1:JunitRunner>
	<android-2_1:DalvikAnnotation rdf:about="&android-2_1;theDalvikAnnotationPart">
	</android-2_1:DalvikAnnotation>
	<android-2_1:DalvikBytecode rdf:about="&android-2_1;theDalvikBytecodePart">
	</android-2_1:DalvikBytecode>
	<android-2_1:DalvikSystem rdf:about="&android-2_1;theDalvikSystemPart">
	</android-2_1:DalvikSystem>
	<owl:Class rdf:about="&android-2_1;AndroidClassLibrary">
		<rdfs:subClassOf rdf:resource="&android-1_6;AndroidClassLibrary"/>
		<rdfs:comment xml:lang="en">JavaLibrary implementing the android package for Android 2.1</rdfs:comment>
		<rdfs:comment xml:lang="OWLManchester">platform:implementsInterface some AndroidAPI</rdfs:comment>
	</owl:Class>
	<owl:Class rdf:about="&android-2_1;AndroidAccessibilityserviceClassLibrary">
		<rdfs:subClassOf rdf:resource="&android-1_6;AndroidAccessibilityserviceClassLibrary"/>
		<rdfs:comment xml:lang="en">JavaLibrary implementing the android.accessibilityservice package for Android 2.1</rdfs:comment>
		<rdfs:comment xml:lang="OWLManchester">platform:implementsInterface some AndroidAccessibilityserviceAPI</rdfs:comment>
	</owl:Class>
	<owl:Class rdf:about="&android-2_1;AndroidAppClassLibrary">
		<rdfs:subClassOf rdf:resource="&android-1_6;AndroidAppClassLibrary"/>
		<rdfs:comment xml:lang="en">JavaLibrary implementing the android.app package for Android 2.1</rdfs:comment>
		<rdfs:comment xml:lang="OWLManchester">platform:implementsInterface some AndroidAppAPI</rdfs:comment>
	</owl:Class>
	<owl:Class rdf:about="&android-2_1;AndroidViewClassLibrary">
		<rdfs:subClassOf rdf:resource="&java;JavaClassLibrary"/>
		<rdfs:comment xml:lang="en">JavaLibrary implementing the android.view package for Android 2.1</rdfs:comment>
		<rdfs:comment xml:lang="OWLManchester">platform:implementsInterface some AndroidViewAPI</rdfs:comment>
	</owl:Class>
	<owl:Class rdf:about="&android-2_1;AndroidViewAccessibilityClassLibrary">
		<owl:equivalentClass rdf:resource="&android-1_6;AndroidViewAccessibilityClassLibrary"/>
		<rdfs:subClassOf rdf:resource="&java;JavaClassLibrary"/>
		<rdfs:comment xml:lang="en">JavaLibrary implementing the android.view.accessibility package for Android 2.1</rdfs:comment>
		<rdfs:comment xml:lang="OWLManchester">platform:implementsInterface some AndroidViewAccessibilityAPI</rdfs:comment>
	</owl:Class>
	<owl:Class rdf:about="&android-2_1;AndroidViewInputmethodClassLibrary">
		<rdfs:subClassOf rdf:resource="&android-1_6;AndroidViewInputmethodClassLibrary"/>
		<rdfs:comment xml:lang="en">JavaLibrary implementing the android.view.inputmethod package for Android 2.1</rdfs:comment>
		<rdfs:comment xml:lang="OWLManchester">platform:implementsInterface some AndroidViewInputmethodAPI</rdfs:comment>
	</owl:Class>
	<owl:Class rdf:about="&android-2_1;AndroidViewAnimationClassLibrary">
		<rdfs:subClassOf rdf:resource="&android-1_6;AndroidViewAnimationClassLibrary"/>
		<rdfs:comment xml:lang="en">JavaLibrary implementing the android.view.animation package for Android 2.1</rdfs:comment>
		<rdfs:comment xml:lang="OWLManchester">platform:implementsInterface some AndroidViewAnimationAPI</rdfs:comment>
	</owl:Class>
	<owl:Class rdf:about="&android-2_1;AndroidContentClassLibrary">
		<rdfs:subClassOf rdf:resource="&android-1_6;AndroidContentClassLibrary"/>
		<rdfs:comment xml:lang="en">JavaLibrary implementing the android.content package for Android 2.1</rdfs:comment>
		<rdfs:comment xml:lang="OWLManchester">platform:implementsInterface some AndroidContentAPI</rdfs:comment>
	</owl:Class>
	<owl:Class rdf:about="&android-2_1;AndroidContentResClassLibrary">
		<rdfs:subClassOf rdf:resource="&android-1_6;AndroidContentResClassLibrary"/>
		<rdfs:comment xml:lang="en">JavaLibrary implementing the android.content.res package for Android 2.1</rdfs:comment>
		<rdfs:comment xml:lang="OWLManchester">platform:implementsInterface some AndroidContentResAPI</rdfs:comment>
	</owl:Class>
	<owl:Class rdf:about="&android-2_1;AndroidContentPmClassLibrary">
		<rdfs:subClassOf rdf:resource="&android-1_6;AndroidContentPmClassLibrary"/>
		<rdfs:comment xml:lang="en">JavaLibrary implementing the android.content.pm package for Android 2.1</rdfs:comment>
		<rdfs:comment xml:lang="OWLManchester">platform:implementsInterface some AndroidContentPmAPI</rdfs:comment>
	</owl:Class>
	<owl:Class rdf:about="&android-2_1;AndroidOsClassLibrary">
		<rdfs:subClassOf rdf:resource="&android-1_6;AndroidOsClassLibrary"/>
		<rdfs:comment xml:lang="en">JavaLibrary implementing the android.os package for Android 2.1</rdfs:comment>
		<rdfs:comment xml:lang="OWLManchester">platform:implementsInterface some AndroidOsAPI</rdfs:comment>
	</owl:Class>
	<owl:Class rdf:about="&android-2_1;AndroidAccountsClassLibrary">
		<rdfs:subClassOf rdf:resource="&java;JavaClassLibrary"/>
		<rdfs:comment xml:lang="en">JavaLibrary implementing the android.accounts package for Android 2.1</rdfs:comment>
		<rdfs:comment xml:lang="OWLManchester">platform:implementsInterface some AndroidAccountsAPI</rdfs:comment>
	</owl:Class>
	<owl:Class rdf:about="&android-2_1;AndroidGraphicsClassLibrary">
		<rdfs:subClassOf rdf:resource="&android-1_6;AndroidGraphicsClassLibrary"/>
		<rdfs:comment xml:lang="en">JavaLibrary implementing the android.graphics package for Android 2.1</rdfs:comment>
		<rdfs:comment xml:lang="OWLManchester">platform:implementsInterface some AndroidGraphicsAPI</rdfs:comment>
	</owl:Class>
	<owl:Class rdf:about="&android-2_1;AndroidGraphicsDrawableClassLibrary">
		<rdfs:subClassOf rdf:resource="&android-1_6;AndroidGraphicsDrawableClassLibrary"/>
		<rdfs:comment xml:lang="en">JavaLibrary implementing the android.graphics.drawable package for Android 2.1</rdfs:comment>
		<rdfs:comment xml:lang="OWLManchester">platform:implementsInterface some AndroidGraphicsDrawableAPI</rdfs:comment>
	</owl:Class>
	<owl:Class rdf:about="&android-2_1;AndroidGraphicsDrawableShapesClassLibrary">
		<owl:equivalentClass rdf:resource="&android-1_6;AndroidGraphicsDrawableShapesClassLibrary"/>
		<rdfs:subClassOf rdf:resource="&java;JavaClassLibrary"/>
		<rdfs:comment xml:lang="en">JavaLibrary implementing the android.graphics.drawable.shapes package for Android 2.1</rdfs:comment>
		<rdfs:comment xml:lang="OWLManchester">platform:implementsInterface some AndroidGraphicsDrawableShapesAPI</rdfs:comment>
	</owl:Class>
	<owl:Class rdf:about="&android-2_1;AndroidNetClassLibrary">
		<owl:equivalentClass rdf:resource="&android-1_6;AndroidNetClassLibrary"/>
		<rdfs:subClassOf rdf:resource="&java;JavaClassLibrary"/>
		<rdfs:comment xml:lang="en">JavaLibrary implementing the android.net package for Android 2.1</rdfs:comment>
		<rdfs:comment xml:lang="OWLManchester">platform:implementsInterface some AndroidNetAPI</rdfs:comment>
	</owl:Class>
	<owl:Class rdf:about="&android-2_1;AndroidNetHttpClassLibrary">
		<owl:equivalentClass rdf:resource="&android-1_6;AndroidNetHttpClassLibrary"/>
		<rdfs:subClassOf rdf:resource="&java;JavaClassLibrary"/>
		<rdfs:comment xml:lang="en">JavaLibrary implementing the android.net.http package for Android 2.1</rdfs:comment>
		<rdfs:comment xml:lang="OWLManchester">platform:implementsInterface some AndroidNetHttpAPI</rdfs:comment>
	</owl:Class>
	<owl:Class rdf:about="&android-2_1;AndroidNetWifiClassLibrary">
		<owl:equivalentClass rdf:resource="&android-1_6;AndroidNetWifiClassLibrary"/>
		<rdfs:subClassOf rdf:resource="&java;JavaClassLibrary"/>
		<rdfs:comment xml:lang="en">JavaLibrary implementing the android.net.wifi package for Android 2.1</rdfs:comment>
		<rdfs:comment xml:lang="OWLManchester">platform:implementsInterface some AndroidNetWifiAPI</rdfs:comment>
	</owl:Class>
	<owl:Class rdf:about="&android-2_1;AndroidDatabaseClassLibrary">
		<rdfs:subClassOf rdf:resource="&android-1_6;AndroidDatabaseClassLibrary"/>
		<rdfs:comment xml:lang="en">JavaLibrary implementing the android.database package for Android 2.1</rdfs:comment>
		<rdfs:comment xml:lang="OWLManchester">platform:implementsInterface some AndroidDatabaseAPI</rdfs:comment>
	</owl:Class>
	<owl:Class rdf:about="&android-2_1;AndroidDatabaseSqliteClassLibrary">
		<rdfs:subClassOf rdf:resource="&android-1_6;AndroidDatabaseSqliteClassLibrary"/>
		<rdfs:comment xml:lang="en">JavaLibrary implementing the android.database.sqlite package for Android 2.1</rdfs:comment>
		<rdfs:comment xml:lang="OWLManchester">platform:implementsInterface some AndroidDatabaseSqliteAPI</rdfs:comment>
	</owl:Class>
	<owl:Class rdf:about="&android-2_1;AndroidUtilClassLibrary">
		<rdfs:subClassOf rdf:resource="&android-1_6;AndroidUtilClassLibrary"/>
		<rdfs:comment xml:lang="en">JavaLibrary implementing the android.util package for Android 2.1</rdfs:comment>
		<rdfs:comment xml:lang="OWLManchester">platform:implementsInterface some AndroidUtilAPI</rdfs:comment>
	</owl:Class>
	<owl:Class rdf:about="&android-2_1;AndroidWidgetClassLibrary">
		<rdfs:subClassOf rdf:resource="&java;JavaClassLibrary"/>
		<rdfs:comment xml:lang="en">JavaLibrary implementing the android.widget package for Android 2.1</rdfs:comment>
		<rdfs:comment xml:lang="OWLManchester">platform:implementsInterface some AndroidWidgetAPI</rdfs:comment>
	</owl:Class>
	<owl:Class rdf:about="&android-2_1;AndroidAppwidgetClassLibrary">
		<rdfs:subClassOf rdf:resource="&java;JavaClassLibrary"/>
		<rdfs:comment xml:lang="en">JavaLibrary implementing the android.appwidget package for Android 2.1</rdfs:comment>
		<rdfs:comment xml:lang="OWLManchester">platform:implementsInterface some AndroidAppwidgetAPI</rdfs:comment>
	</owl:Class>
	<owl:Class rdf:about="&android-2_1;AndroidBluetoothClassLibrary">
		<rdfs:subClassOf rdf:resource="&java;JavaClassLibrary"/>
		<rdfs:comment xml:lang="en">JavaLibrary implementing the android.bluetooth package for Android 2.1</rdfs:comment>
		<rdfs:comment xml:lang="OWLManchester">platform:implementsInterface some AndroidBluetoothAPI</rdfs:comment>
	</owl:Class>
	<owl:Class rdf:about="&android-2_1;AndroidGestureClassLibrary">
		<rdfs:subClassOf rdf:resource="&java;JavaClassLibrary"/>
		<rdfs:comment xml:lang="en">JavaLibrary implementing the android.gesture package for Android 2.1</rdfs:comment>
		<rdfs:comment xml:lang="OWLManchester">platform:implementsInterface some AndroidGestureAPI</rdfs:comment>
	</owl:Class>
	<owl:Class rdf:about="&android-2_1;AndroidHardwareClassLibrary">
		<rdfs:subClassOf rdf:resource="&android-1_6;AndroidHardwareClassLibrary"/>
		<rdfs:comment xml:lang="en">JavaLibrary implementing the android.hardware package for Android 2.1</rdfs:comment>
		<rdfs:comment xml:lang="OWLManchester">platform:implementsInterface some AndroidHardwareAPI</rdfs:comment>
	</owl:Class>
	<owl:Class rdf:about="&android-2_1;AndroidInputmethodserviceClassLibrary">
		<rdfs:subClassOf rdf:resource="&android-1_6;AndroidInputmethodserviceClassLibrary"/>
		<rdfs:comment xml:lang="en">JavaLibrary implementing the android.inputmethodservice package for Android 2.1</rdfs:comment>
		<rdfs:comment xml:lang="OWLManchester">platform:implementsInterface some AndroidInputmethodserviceAPI</rdfs:comment>
	</owl:Class>
	<owl:Class rdf:about="&android-2_1;AndroidLocationClassLibrary">
		<rdfs:subClassOf rdf:resource="&android-1_6;AndroidLocationClassLibrary"/>
		<rdfs:comment xml:lang="en">JavaLibrary implementing the android.location package for Android 2.1</rdfs:comment>
		<rdfs:comment xml:lang="OWLManchester">platform:implementsInterface some AndroidLocationAPI</rdfs:comment>
	</owl:Class>
	<owl:Class rdf:about="&android-2_1;AndroidMediaClassLibrary">
		<rdfs:subClassOf rdf:resource="&android-1_6;AndroidMediaClassLibrary"/>
		<rdfs:comment xml:lang="en">JavaLibrary implementing the android.media package for Android 2.1</rdfs:comment>
		<rdfs:comment xml:lang="OWLManchester">platform:implementsInterface some AndroidMediaAPI</rdfs:comment>
	</owl:Class>
	<owl:Class rdf:about="&android-2_1;AndroidOpenglClassLibrary">
		<rdfs:subClassOf rdf:resource="&android-1_6;AndroidOpenglClassLibrary"/>
		<rdfs:comment xml:lang="en">JavaLibrary implementing the android.opengl package for Android 2.1</rdfs:comment>
		<rdfs:comment xml:lang="OWLManchester">platform:implementsInterface some AndroidOpenglAPI</rdfs:comment>
	</owl:Class>
	<owl:Class rdf:about="&android-2_1;AndroidPreferenceClassLibrary">
		<rdfs:subClassOf rdf:resource="&android-1_6;AndroidPreferenceClassLibrary"/>
		<rdfs:comment xml:lang="en">JavaLibrary implementing the android.preference package for Android 2.1</rdfs:comment>
		<rdfs:comment xml:lang="OWLManchester">platform:implementsInterface some AndroidPreferenceAPI</rdfs:comment>
	</owl:Class>
	<owl:Class rdf:about="&android-2_1;AndroidProviderClassLibrary">
		<rdfs:subClassOf rdf:resource="&android-1_6;AndroidProviderClassLibrary"/>
		<rdfs:comment xml:lang="en">JavaLibrary implementing the android.provider package for Android 2.1</rdfs:comment>
		<rdfs:comment xml:lang="OWLManchester">platform:implementsInterface some AndroidProviderAPI</rdfs:comment>
	</owl:Class>
	<owl:Class rdf:about="&android-2_1;AndroidWebkitClassLibrary">
		<rdfs:subClassOf rdf:resource="&java;JavaClassLibrary"/>
		<rdfs:comment xml:lang="en">JavaLibrary implementing the android.webkit package for Android 2.1</rdfs:comment>
		<rdfs:comment xml:lang="OWLManchester">platform:implementsInterface some AndroidWebkitAPI</rdfs:comment>
	</owl:Class>
	<owl:Class rdf:about="&android-2_1;AndroidSaxClassLibrary">
		<owl:equivalentClass rdf:resource="&android-1_6;AndroidSaxClassLibrary"/>
		<rdfs:subClassOf rdf:resource="&java;JavaClassLibrary"/>
		<rdfs:comment xml:lang="en">JavaLibrary implementing the android.sax package for Android 2.1</rdfs:comment>
		<rdfs:comment xml:lang="OWLManchester">platform:implementsInterface some AndroidSaxAPI</rdfs:comment>
	</owl:Class>
	<owl:Class rdf:about="&android-2_1;AndroidServiceWallpaperClassLibrary">
		<rdfs:subClassOf rdf:resource="&java;JavaClassLibrary"/>
		<rdfs:comment xml:lang="en">JavaLibrary implementing the android.service.wallpaper package for Android 2.1</rdfs:comment>
		<rdfs:comment xml:lang="OWLManchester">platform:implementsInterface some AndroidServiceWallpaperAPI</rdfs:comment>
	</owl:Class>
	<owl:Class rdf:about="&android-2_1;AndroidSpeechClassLibrary">
		<owl:equivalentClass rdf:resource="&android-1_6;AndroidSpeechClassLibrary"/>
		<rdfs:subClassOf rdf:resource="&java;JavaClassLibrary"/>
		<rdfs:comment xml:lang="en">JavaLibrary implementing the android.speech package for Android 2.1</rdfs:comment>
		<rdfs:comment xml:lang="OWLManchester">platform:implementsInterface some AndroidSpeechAPI</rdfs:comment>
	</owl:Class>
	<owl:Class rdf:about="&android-2_1;AndroidSpeechTtsClassLibrary">
		<owl:equivalentClass rdf:resource="&android-1_6;AndroidSpeechTtsClassLibrary"/>
		<rdfs:subClassOf rdf:resource="&java;JavaClassLibrary"/>
		<rdfs:comment xml:lang="en">JavaLibrary implementing the android.speech.tts package for Android 2.1</rdfs:comment>
		<rdfs:comment xml:lang="OWLManchester">platform:implementsInterface some AndroidSpeechTtsAPI</rdfs:comment>
	</owl:Class>
	<owl:Class rdf:about="&android-2_1;AndroidTelephonyClassLibrary">
		<rdfs:subClassOf rdf:resource="&android-1_6;AndroidTelephonyClassLibrary"/>
		<rdfs:comment xml:lang="en">JavaLibrary implementing the android.telephony package for Android 2.1</rdfs:comment>
		<rdfs:comment xml:lang="OWLManchester">platform:implementsInterface some AndroidTelephonyAPI</rdfs:comment>
	</owl:Class>
	<owl:Class rdf:about="&android-2_1;AndroidTelephonyCdmaClassLibrary">
		<rdfs:subClassOf rdf:resource="&java;JavaClassLibrary"/>
		<rdfs:comment xml:lang="en">JavaLibrary implementing the android.telephony.cdma package for Android 2.1</rdfs:comment>
		<rdfs:comment xml:lang="OWLManchester">platform:implementsInterface some AndroidTelephonyCdmaAPI</rdfs:comment>
	</owl:Class>
	<owl:Class rdf:about="&android-2_1;AndroidTelephonyGsmClassLibrary">
		<owl:equivalentClass rdf:resource="&android-1_6;AndroidTelephonyGsmClassLibrary"/>
		<rdfs:subClassOf rdf:resource="&java;JavaClassLibrary"/>
		<rdfs:comment xml:lang="en">JavaLibrary implementing the android.telephony.gsm package for Android 2.1</rdfs:comment>
		<rdfs:comment xml:lang="OWLManchester">platform:implementsInterface some AndroidTelephonyGsmAPI</rdfs:comment>
	</owl:Class>
	<owl:Class rdf:about="&android-2_1;AndroidTextClassLibrary">
		<rdfs:subClassOf rdf:resource="&android-1_6;AndroidTextClassLibrary"/>
		<rdfs:comment xml:lang="en">JavaLibrary implementing the android.text package for Android 2.1</rdfs:comment>
		<rdfs:comment xml:lang="OWLManchester">platform:implementsInterface some AndroidTextAPI</rdfs:comment>
	</owl:Class>
	<owl:Class rdf:about="&android-2_1;AndroidTextFormatClassLibrary">
		<rdfs:subClassOf rdf:resource="&android-1_6;AndroidTextFormatClassLibrary"/>
		<rdfs:comment xml:lang="en">JavaLibrary implementing the android.text.format package for Android 2.1</rdfs:comment>
		<rdfs:comment xml:lang="OWLManchester">platform:implementsInterface some AndroidTextFormatAPI</rdfs:comment>
	</owl:Class>
	<owl:Class rdf:about="&android-2_1;AndroidTextMethodClassLibrary">
		<rdfs:subClassOf rdf:resource="&android-1_6;AndroidTextMethodClassLibrary"/>
		<rdfs:comment xml:lang="en">JavaLibrary implementing the android.text.method package for Android 2.1</rdfs:comment>
		<rdfs:comment xml:lang="OWLManchester">platform:implementsInterface some AndroidTextMethodAPI</rdfs:comment>
	</owl:Class>
	<owl:Class rdf:about="&android-2_1;AndroidTextStyleClassLibrary">
		<rdfs:subClassOf rdf:resource="&android-1_6;AndroidTextStyleClassLibrary"/>
		<rdfs:comment xml:lang="en">JavaLibrary implementing the android.text.style package for Android 2.1</rdfs:comment>
		<rdfs:comment xml:lang="OWLManchester">platform:implementsInterface some AndroidTextStyleAPI</rdfs:comment>
	</owl:Class>
	<owl:Class rdf:about="&android-2_1;AndroidTextUtilClassLibrary">
		<owl:equivalentClass rdf:resource="&android-1_6;AndroidTextUtilClassLibrary"/>
		<rdfs:subClassOf rdf:resource="&java;JavaClassLibrary"/>
		<rdfs:comment xml:lang="en">JavaLibrary implementing the android.text.util package for Android 2.1</rdfs:comment>
		<rdfs:comment xml:lang="OWLManchester">platform:implementsInterface some AndroidTextUtilAPI</rdfs:comment>
	</owl:Class>
	<owl:Class rdf:about="&android-2_1;AndroidTestClassLibrary">
		<rdfs:subClassOf rdf:resource="&android-1_6;AndroidTestClassLibrary"/>
		<rdfs:comment xml:lang="en">JavaLibrary implementing the android.test package for Android 2.1</rdfs:comment>
		<rdfs:comment xml:lang="OWLManchester">platform:implementsInterface some AndroidTestAPI</rdfs:comment>
	</owl:Class>
	<owl:Class rdf:about="&android-2_1;AndroidTestMockClassLibrary">
		<rdfs:subClassOf rdf:resource="&android-1_6;AndroidTestMockClassLibrary"/>
		<rdfs:comment xml:lang="en">JavaLibrary implementing the android.test.mock package for Android 2.1</rdfs:comment>
		<rdfs:comment xml:lang="OWLManchester">platform:implementsInterface some AndroidTestMockAPI</rdfs:comment>
	</owl:Class>
	<owl:Class rdf:about="&android-2_1;AndroidTestSuitebuilderClassLibrary">
		<owl:equivalentClass rdf:resource="&android-1_6;AndroidTestSuitebuilderClassLibrary"/>
		<rdfs:subClassOf rdf:resource="&java;JavaClassLibrary"/>
		<rdfs:comment xml:lang="en">JavaLibrary implementing the android.test.suitebuilder package for Android 2.1</rdfs:comment>
		<rdfs:comment xml:lang="OWLManchester">platform:implementsInterface some AndroidTestSuitebuilderAPI</rdfs:comment>
	</owl:Class>
	<owl:Class rdf:about="&android-2_1;AndroidTestSuitebuilderAnnotationClassLibrary">
		<owl:equivalentClass rdf:resource="&android-1_6;AndroidTestSuitebuilderAnnotationClassLibrary"/>
		<rdfs:subClassOf rdf:resource="&java;JavaClassLibrary"/>
		<rdfs:comment xml:lang="en">JavaLibrary implementing the android.test.suitebuilder.annotation package for Android 2.1</rdfs:comment>
		<rdfs:comment xml:lang="OWLManchester">platform:implementsInterface some AndroidTestSuitebuilderAnnotationAPI</rdfs:comment>
	</owl:Class>
	<owl:Class rdf:about="&android-2_1;JavaLangClassLibrary">
		<owl:equivalentClass rdf:resource="&android-1_6;JavaLangClassLibrary"/>
		<rdfs:subClassOf rdf:resource="&java;JavaClassLibrary"/>
		<rdfs:comment xml:lang="en">JavaLibrary implementing the java.lang package for Android 2.1</rdfs:comment>
		<rdfs:comment xml:lang="OWLManchester">platform:implementsInterface some JavaLangAPI</rdfs:comment>
	</owl:Class>
	<owl:Class rdf:about="&android-2_1;JavaLangAnnotationClassLibrary">
		<owl:equivalentClass rdf:resource="&android-1_6;JavaLangAnnotationClassLibrary"/>
		<rdfs:subClassOf rdf:resource="&java;JavaClassLibrary"/>
		<rdfs:comment xml:lang="en">JavaLibrary implementing the java.lang.annotation package for Android 2.1</rdfs:comment>
		<rdfs:comment xml:lang="OWLManchester">platform:implementsInterface some JavaLangAnnotationAPI</rdfs:comment>
	</owl:Class>
	<owl:Class rdf:about="&android-2_1;JavaLangReflectClassLibrary">
		<owl:equivalentClass rdf:resource="&java-se-6;JavaLangReflectClassLibrary"/>
		<owl:equivalentClass rdf:resource="&android-1_6;JavaLangReflectClassLibrary"/>
		<rdfs:subClassOf rdf:resource="&java;JavaClassLibrary"/>
		<rdfs:comment xml:lang="en">JavaLibrary implementing the java.lang.reflect package for Android 2.1</rdfs:comment>
		<rdfs:comment xml:lang="OWLManchester">platform:implementsInterface some JavaLangReflectAPI</rdfs:comment>
	</owl:Class>
	<owl:Class rdf:about="&android-2_1;JavaLangRefClassLibrary">
		<owl:equivalentClass rdf:resource="&java-se-6;JavaLangRefClassLibrary"/>
		<owl:equivalentClass rdf:resource="&android-1_6;JavaLangRefClassLibrary"/>
		<rdfs:subClassOf rdf:resource="&java;JavaClassLibrary"/>
		<rdfs:comment xml:lang="en">JavaLibrary implementing the java.lang.ref package for Android 2.1</rdfs:comment>
		<rdfs:comment xml:lang="OWLManchester">platform:implementsInterface some JavaLangRefAPI</rdfs:comment>
	</owl:Class>
	<owl:Class rdf:about="&android-2_1;JavaUtilClassLibrary">
		<owl:equivalentClass rdf:resource="&android-1_6;JavaUtilClassLibrary"/>
		<rdfs:subClassOf rdf:resource="&java;JavaClassLibrary"/>
		<rdfs:comment xml:lang="en">JavaLibrary implementing the java.util package for Android 2.1</rdfs:comment>
		<rdfs:comment xml:lang="OWLManchester">platform:implementsInterface some JavaUtilAPI</rdfs:comment>
	</owl:Class>
	<owl:Class rdf:about="&android-2_1;JavaUtilConcurrentClassLibrary">
		<owl:equivalentClass rdf:resource="&android-1_6;JavaUtilConcurrentClassLibrary"/>
		<rdfs:subClassOf rdf:resource="&java;JavaClassLibrary"/>
		<rdfs:comment xml:lang="en">JavaLibrary implementing the java.util.concurrent package for Android 2.1</rdfs:comment>
		<rdfs:comment xml:lang="OWLManchester">platform:implementsInterface some JavaUtilConcurrentAPI</rdfs:comment>
	</owl:Class>
	<owl:Class rdf:about="&android-2_1;JavaUtilConcurrentAtomicClassLibrary">
		<owl:equivalentClass rdf:resource="&android-1_6;JavaUtilConcurrentAtomicClassLibrary"/>
		<rdfs:subClassOf rdf:resource="&java;JavaClassLibrary"/>
		<rdfs:comment xml:lang="en">JavaLibrary implementing the java.util.concurrent.atomic package for Android 2.1</rdfs:comment>
		<rdfs:comment xml:lang="OWLManchester">platform:implementsInterface some JavaUtilConcurrentAtomicAPI</rdfs:comment>
	</owl:Class>
	<owl:Class rdf:about="&android-2_1;JavaUtilConcurrentLocksClassLibrary">
		<rdfs:subClassOf rdf:resource="&android-1_6;JavaUtilConcurrentLocksClassLibrary"/>
		<rdfs:comment xml:lang="en">JavaLibrary implementing the java.util.concurrent.locks package for Android 2.1</rdfs:comment>
		<rdfs:comment xml:lang="OWLManchester">platform:implementsInterface some JavaUtilConcurrentLocksAPI</rdfs:comment>
	</owl:Class>
	<owl:Class rdf:about="&android-2_1;JavaUtilRegexClassLibrary">
		<owl:equivalentClass rdf:resource="&java-se-6;JavaUtilRegexClassLibrary"/>
		<owl:equivalentClass rdf:resource="&android-1_6;JavaUtilRegexClassLibrary"/>
		<rdfs:subClassOf rdf:resource="&java;JavaClassLibrary"/>
		<rdfs:comment xml:lang="en">JavaLibrary implementing the java.util.regex package for Android 2.1</rdfs:comment>
		<rdfs:comment xml:lang="OWLManchester">platform:implementsInterface some JavaUtilRegexAPI</rdfs:comment>
	</owl:Class>
	<owl:Class rdf:about="&android-2_1;JavaUtilJarClassLibrary">
		<owl:equivalentClass rdf:resource="&java-se-6;JavaUtilJarClassLibrary"/>
		<owl:equivalentClass rdf:resource="&android-1_6;JavaUtilJarClassLibrary"/>
		<rdfs:subClassOf rdf:resource="&java;JavaClassLibrary"/>
		<rdfs:comment xml:lang="en">JavaLibrary implementing the java.util.jar package for Android 2.1</rdfs:comment>
		<rdfs:comment xml:lang="OWLManchester">platform:implementsInterface some JavaUtilJarAPI</rdfs:comment>
	</owl:Class>
	<owl:Class rdf:about="&android-2_1;JavaUtilZipClassLibrary">
		<owl:equivalentClass rdf:resource="&android-1_6;JavaUtilZipClassLibrary"/>
		<rdfs:subClassOf rdf:resource="&java;JavaClassLibrary"/>
		<rdfs:comment xml:lang="en">JavaLibrary implementing the java.util.zip package for Android 2.1</rdfs:comment>
		<rdfs:comment xml:lang="OWLManchester">platform:implementsInterface some JavaUtilZipAPI</rdfs:comment>
	</owl:Class>
	<owl:Class rdf:about="&android-2_1;JavaUtilLoggingClassLibrary">
		<owl:equivalentClass rdf:resource="&android-1_6;JavaUtilLoggingClassLibrary"/>
		<rdfs:subClassOf rdf:resource="&java;JavaClassLibrary"/>
		<rdfs:comment xml:lang="en">JavaLibrary implementing the java.util.logging package for Android 2.1</rdfs:comment>
		<rdfs:comment xml:lang="OWLManchester">platform:implementsInterface some JavaUtilLoggingAPI</rdfs:comment>
	</owl:Class>
	<owl:Class rdf:about="&android-2_1;JavaUtilPrefsClassLibrary">
		<owl:equivalentClass rdf:resource="&java-se-6;JavaUtilPrefsClassLibrary"/>
		<owl:equivalentClass rdf:resource="&android-1_6;JavaUtilPrefsClassLibrary"/>
		<rdfs:subClassOf rdf:resource="&java;JavaClassLibrary"/>
		<rdfs:comment xml:lang="en">JavaLibrary implementing the java.util.prefs package for Android 2.1</rdfs:comment>
		<rdfs:comment xml:lang="OWLManchester">platform:implementsInterface some JavaUtilPrefsAPI</rdfs:comment>
	</owl:Class>
	<owl:Class rdf:about="&android-2_1;JavaIoClassLibrary">
		<owl:equivalentClass rdf:resource="&android-1_6;JavaIoClassLibrary"/>
		<rdfs:subClassOf rdf:resource="&java;JavaClassLibrary"/>
		<rdfs:comment xml:lang="en">JavaLibrary implementing the java.io package for Android 2.1</rdfs:comment>
		<rdfs:comment xml:lang="OWLManchester">platform:implementsInterface some JavaIoAPI</rdfs:comment>
	</owl:Class>
	<owl:Class rdf:about="&android-2_1;JavaNioClassLibrary">
		<owl:equivalentClass rdf:resource="&android-1_6;JavaNioClassLibrary"/>
		<rdfs:subClassOf rdf:resource="&java;JavaClassLibrary"/>
		<rdfs:comment xml:lang="en">JavaLibrary implementing the java.nio package for Android 2.1</rdfs:comment>
		<rdfs:comment xml:lang="OWLManchester">platform:implementsInterface some JavaNioAPI</rdfs:comment>
	</owl:Class>
	<owl:Class rdf:about="&android-2_1;JavaNioChannelsClassLibrary">
		<owl:equivalentClass rdf:resource="&java-se-6;JavaNioChannelsClassLibrary"/>
		<owl:equivalentClass rdf:resource="&android-1_6;JavaNioChannelsClassLibrary"/>
		<rdfs:subClassOf rdf:resource="&java;JavaClassLibrary"/>
		<rdfs:comment xml:lang="en">JavaLibrary implementing the java.nio.channels package for Android 2.1</rdfs:comment>
		<rdfs:comment xml:lang="OWLManchester">platform:implementsInterface some JavaNioChannelsAPI</rdfs:comment>
	</owl:Class>
	<owl:Class rdf:about="&android-2_1;JavaNioChannelsSpiClassLibrary">
		<owl:equivalentClass rdf:resource="&java-se-6;JavaNioChannelsSpiClassLibrary"/>
		<owl:equivalentClass rdf:resource="&android-1_6;JavaNioChannelsSpiClassLibrary"/>
		<rdfs:subClassOf rdf:resource="&java;JavaClassLibrary"/>
		<rdfs:comment xml:lang="en">JavaLibrary implementing the java.nio.channels.spi package for Android 2.1</rdfs:comment>
		<rdfs:comment xml:lang="OWLManchester">platform:implementsInterface some JavaNioChannelsSpiAPI</rdfs:comment>
	</owl:Class>
	<owl:Class rdf:about="&android-2_1;JavaNioCharsetClassLibrary">
		<owl:equivalentClass rdf:resource="&java-se-6;JavaNioCharsetClassLibrary"/>
		<owl:equivalentClass rdf:resource="&android-1_6;JavaNioCharsetClassLibrary"/>
		<rdfs:subClassOf rdf:resource="&java;JavaClassLibrary"/>
		<rdfs:comment xml:lang="en">JavaLibrary implementing the java.nio.charset package for Android 2.1</rdfs:comment>
		<rdfs:comment xml:lang="OWLManchester">platform:implementsInterface some JavaNioCharsetAPI</rdfs:comment>
	</owl:Class>
	<owl:Class rdf:about="&android-2_1;JavaNioCharsetSpiClassLibrary">
		<owl:equivalentClass rdf:resource="&java-se-6;JavaNioCharsetSpiClassLibrary"/>
		<owl:equivalentClass rdf:resource="&android-1_6;JavaNioCharsetSpiClassLibrary"/>
		<rdfs:subClassOf rdf:resource="&java;JavaClassLibrary"/>
		<rdfs:comment xml:lang="en">JavaLibrary implementing the java.nio.charset.spi package for Android 2.1</rdfs:comment>
		<rdfs:comment xml:lang="OWLManchester">platform:implementsInterface some JavaNioCharsetSpiAPI</rdfs:comment>
	</owl:Class>
	<owl:Class rdf:about="&android-2_1;JavaNetClassLibrary">
		<owl:equivalentClass rdf:resource="&android-1_6;JavaNetClassLibrary"/>
		<rdfs:subClassOf rdf:resource="&java;JavaClassLibrary"/>
		<rdfs:comment xml:lang="en">JavaLibrary implementing the java.net package for Android 2.1</rdfs:comment>
		<rdfs:comment xml:lang="OWLManchester">platform:implementsInterface some JavaNetAPI</rdfs:comment>
	</owl:Class>
	<owl:Class rdf:about="&android-2_1;JavaSecurityClassLibrary">
		<owl:equivalentClass rdf:resource="&android-1_6;JavaSecurityClassLibrary"/>
		<rdfs:subClassOf rdf:resource="&java;JavaClassLibrary"/>
		<rdfs:comment xml:lang="en">JavaLibrary implementing the java.security package for Android 2.1</rdfs:comment>
		<rdfs:comment xml:lang="OWLManchester">platform:implementsInterface some JavaSecurityAPI</rdfs:comment>
	</owl:Class>
	<owl:Class rdf:about="&android-2_1;JavaSecurityCertClassLibrary">
		<owl:equivalentClass rdf:resource="&java-se-6;JavaSecurityCertClassLibrary"/>
		<owl:equivalentClass rdf:resource="&android-1_6;JavaSecurityCertClassLibrary"/>
		<rdfs:subClassOf rdf:resource="&java;JavaClassLibrary"/>
		<rdfs:comment xml:lang="en">JavaLibrary implementing the java.security.cert package for Android 2.1</rdfs:comment>
		<rdfs:comment xml:lang="OWLManchester">platform:implementsInterface some JavaSecurityCertAPI</rdfs:comment>
	</owl:Class>
	<owl:Class rdf:about="&android-2_1;JavaSecuritySpecClassLibrary">
		<owl:equivalentClass rdf:resource="&java-se-6;JavaSecuritySpecClassLibrary"/>
		<owl:equivalentClass rdf:resource="&android-1_6;JavaSecuritySpecClassLibrary"/>
		<rdfs:subClassOf rdf:resource="&java;JavaClassLibrary"/>
		<rdfs:comment xml:lang="en">JavaLibrary implementing the java.security.spec package for Android 2.1</rdfs:comment>
		<rdfs:comment xml:lang="OWLManchester">platform:implementsInterface some JavaSecuritySpecAPI</rdfs:comment>
	</owl:Class>
	<owl:Class rdf:about="&android-2_1;JavaSecurityAclClassLibrary">
		<owl:equivalentClass rdf:resource="&java-se-6;JavaSecurityAclClassLibrary"/>
		<owl:equivalentClass rdf:resource="&android-1_6;JavaSecurityAclClassLibrary"/>
		<rdfs:subClassOf rdf:resource="&java;JavaClassLibrary"/>
		<rdfs:comment xml:lang="en">JavaLibrary implementing the java.security.acl package for Android 2.1</rdfs:comment>
		<rdfs:comment xml:lang="OWLManchester">platform:implementsInterface some JavaSecurityAclAPI</rdfs:comment>
	</owl:Class>
	<owl:Class rdf:about="&android-2_1;JavaSecurityInterfacesClassLibrary">
		<owl:equivalentClass rdf:resource="&java-se-6;JavaSecurityInterfacesClassLibrary"/>
		<owl:equivalentClass rdf:resource="&android-1_6;JavaSecurityInterfacesClassLibrary"/>
		<rdfs:subClassOf rdf:resource="&java;JavaClassLibrary"/>
		<rdfs:comment xml:lang="en">JavaLibrary implementing the java.security.interfaces package for Android 2.1</rdfs:comment>
		<rdfs:comment xml:lang="OWLManchester">platform:implementsInterface some JavaSecurityInterfacesAPI</rdfs:comment>
	</owl:Class>
	<owl:Class rdf:about="&android-2_1;JavaTextClassLibrary">
		<owl:equivalentClass rdf:resource="&android-1_6;JavaTextClassLibrary"/>
		<rdfs:subClassOf rdf:resource="&java;JavaClassLibrary"/>
		<rdfs:comment xml:lang="en">JavaLibrary implementing the java.text package for Android 2.1</rdfs:comment>
		<rdfs:comment xml:lang="OWLManchester">platform:implementsInterface some JavaTextAPI</rdfs:comment>
	</owl:Class>
	<owl:Class rdf:about="&android-2_1;JavaAwtFontClassLibrary">
		<owl:equivalentClass rdf:resource="&android-1_6;JavaAwtFontClassLibrary"/>
		<rdfs:subClassOf rdf:resource="&java;JavaClassLibrary"/>
		<rdfs:comment xml:lang="en">JavaLibrary implementing the java.awt.font package for Android 2.1</rdfs:comment>
		<rdfs:comment xml:lang="OWLManchester">platform:implementsInterface some JavaAwtFontAPI</rdfs:comment>
	</owl:Class>
	<owl:Class rdf:about="&android-2_1;JavaBeansClassLibrary">
		<owl:equivalentClass rdf:resource="&android-1_6;JavaBeansClassLibrary"/>
		<rdfs:subClassOf rdf:resource="&java;JavaClassLibrary"/>
		<rdfs:comment xml:lang="en">JavaLibrary implementing the java.beans package for Android 2.1</rdfs:comment>
		<rdfs:comment xml:lang="OWLManchester">platform:implementsInterface some JavaBeansAPI</rdfs:comment>
	</owl:Class>
	<owl:Class rdf:about="&android-2_1;JavaMathClassLibrary">
		<owl:equivalentClass rdf:resource="&android-1_6;JavaMathClassLibrary"/>
		<rdfs:subClassOf rdf:resource="&java;JavaClassLibrary"/>
		<rdfs:comment xml:lang="en">JavaLibrary implementing the java.math package for Android 2.1</rdfs:comment>
		<rdfs:comment xml:lang="OWLManchester">platform:implementsInterface some JavaMathAPI</rdfs:comment>
	</owl:Class>
	<owl:Class rdf:about="&android-2_1;JavaSqlClassLibrary">
		<owl:equivalentClass rdf:resource="&android-1_6;JavaSqlClassLibrary"/>
		<rdfs:subClassOf rdf:resource="&java;JavaClassLibrary"/>
		<rdfs:comment xml:lang="en">JavaLibrary implementing the java.sql package for Android 2.1</rdfs:comment>
		<rdfs:comment xml:lang="OWLManchester">platform:implementsInterface some JavaSqlAPI</rdfs:comment>
	</owl:Class>
	<owl:Class rdf:about="&android-2_1;OrgXmlpullV1ClassLibrary">
		<owl:equivalentClass rdf:resource="&android-1_6;OrgXmlpullV1ClassLibrary"/>
		<rdfs:subClassOf rdf:resource="&java;JavaClassLibrary"/>
		<rdfs:comment xml:lang="en">JavaLibrary implementing the org.xmlpull.v1 package for Android 2.1</rdfs:comment>
		<rdfs:comment xml:lang="OWLManchester">platform:implementsInterface some OrgXmlpullV1API</rdfs:comment>
	</owl:Class>
	<owl:Class rdf:about="&android-2_1;OrgXmlpullV1Sax2ClassLibrary">
		<owl:equivalentClass rdf:resource="&android-1_6;OrgXmlpullV1Sax2ClassLibrary"/>
		<rdfs:subClassOf rdf:resource="&java;JavaClassLibrary"/>
		<rdfs:comment xml:lang="en">JavaLibrary implementing the org.xmlpull.v1.sax2 package for Android 2.1</rdfs:comment>
		<rdfs:comment xml:lang="OWLManchester">platform:implementsInterface some OrgXmlpullV1Sax2API</rdfs:comment>
	</owl:Class>
	<owl:Class rdf:about="&android-2_1;OrgXmlSaxClassLibrary">
		<owl:equivalentClass rdf:resource="&java-se-6;OrgXmlSaxClassLibrary"/>
		<owl:equivalentClass rdf:resource="&android-1_6;OrgXmlSaxClassLibrary"/>
		<rdfs:subClassOf rdf:resource="&java;JavaClassLibrary"/>
		<rdfs:comment xml:lang="en">JavaLibrary implementing the org.xml.sax package for Android 2.1</rdfs:comment>
		<rdfs:comment xml:lang="OWLManchester">platform:implementsInterface some OrgXmlSaxAPI</rdfs:comment>
	</owl:Class>
	<owl:Class rdf:about="&android-2_1;OrgXmlSaxHelpersClassLibrary">
		<owl:equivalentClass rdf:resource="&java-se-6;OrgXmlSaxHelpersClassLibrary"/>
		<owl:equivalentClass rdf:resource="&android-1_6;OrgXmlSaxHelpersClassLibrary"/>
		<rdfs:subClassOf rdf:resource="&java;JavaClassLibrary"/>
		<rdfs:comment xml:lang="en">JavaLibrary implementing the org.xml.sax.helpers package for Android 2.1</rdfs:comment>
		<rdfs:comment xml:lang="OWLManchester">platform:implementsInterface some OrgXmlSaxHelpersAPI</rdfs:comment>
	</owl:Class>
	<owl:Class rdf:about="&android-2_1;OrgXmlSaxExtClassLibrary">
		<owl:equivalentClass rdf:resource="&java-se-6;OrgXmlSaxExtClassLibrary"/>
		<owl:equivalentClass rdf:resource="&android-1_6;OrgXmlSaxExtClassLibrary"/>
		<rdfs:subClassOf rdf:resource="&java;JavaClassLibrary"/>
		<rdfs:comment xml:lang="en">JavaLibrary implementing the org.xml.sax.ext package for Android 2.1</rdfs:comment>
		<rdfs:comment xml:lang="OWLManchester">platform:implementsInterface some OrgXmlSaxExtAPI</rdfs:comment>
	</owl:Class>
	<owl:Class rdf:about="&android-2_1;OrgW3cDomClassLibrary">
		<owl:equivalentClass rdf:resource="&android-1_6;OrgW3cDomClassLibrary"/>
		<rdfs:subClassOf rdf:resource="&java;JavaClassLibrary"/>
		<rdfs:comment xml:lang="en">JavaLibrary implementing the org.w3c.dom package for Android 2.1</rdfs:comment>
		<rdfs:comment xml:lang="OWLManchester">platform:implementsInterface some OrgW3cDomAPI</rdfs:comment>
	</owl:Class>
	<owl:Class rdf:about="&android-2_1;OrgApacheCommonsLoggingClassLibrary">
		<owl:equivalentClass rdf:resource="&android-1_6;OrgApacheCommonsLoggingClassLibrary"/>
		<rdfs:subClassOf rdf:resource="&java;JavaClassLibrary"/>
		<rdfs:comment xml:lang="en">JavaLibrary implementing the org.apache.commons.logging package for Android 2.1</rdfs:comment>
		<rdfs:comment xml:lang="OWLManchester">platform:implementsInterface some OrgApacheCommonsLoggingAPI</rdfs:comment>
	</owl:Class>
	<owl:Class rdf:about="&android-2_1;OrgApacheHttpClassLibrary">
		<owl:equivalentClass rdf:resource="&android-1_6;OrgApacheHttpClassLibrary"/>
		<rdfs:subClassOf rdf:resource="&java;JavaClassLibrary"/>
		<rdfs:comment xml:lang="en">JavaLibrary implementing the org.apache.http package for Android 2.1</rdfs:comment>
		<rdfs:comment xml:lang="OWLManchester">platform:implementsInterface some OrgApacheHttpAPI</rdfs:comment>
	</owl:Class>
	<owl:Class rdf:about="&android-2_1;OrgApacheHttpProtocolClassLibrary">
		<owl:equivalentClass rdf:resource="&android-1_6;OrgApacheHttpProtocolClassLibrary"/>
		<rdfs:subClassOf rdf:resource="&java;JavaClassLibrary"/>
		<rdfs:comment xml:lang="en">JavaLibrary implementing the org.apache.http.protocol package for Android 2.1</rdfs:comment>
		<rdfs:comment xml:lang="OWLManchester">platform:implementsInterface some OrgApacheHttpProtocolAPI</rdfs:comment>
	</owl:Class>
	<owl:Class rdf:about="&android-2_1;OrgApacheHttpUtilClassLibrary">
		<owl:equivalentClass rdf:resource="&android-1_6;OrgApacheHttpUtilClassLibrary"/>
		<rdfs:subClassOf rdf:resource="&java;JavaClassLibrary"/>
		<rdfs:comment xml:lang="en">JavaLibrary implementing the org.apache.http.util package for Android 2.1</rdfs:comment>
		<rdfs:comment xml:lang="OWLManchester">platform:implementsInterface some OrgApacheHttpUtilAPI</rdfs:comment>
	</owl:Class>
	<owl:Class rdf:about="&android-2_1;OrgApacheHttpParamsClassLibrary">
		<owl:equivalentClass rdf:resource="&android-1_6;OrgApacheHttpParamsClassLibrary"/>
		<rdfs:subClassOf rdf:resource="&java;JavaClassLibrary"/>
		<rdfs:comment xml:lang="en">JavaLibrary implementing the org.apache.http.params package for Android 2.1</rdfs:comment>
		<rdfs:comment xml:lang="OWLManchester">platform:implementsInterface some OrgApacheHttpParamsAPI</rdfs:comment>
	</owl:Class>
	<owl:Class rdf:about="&android-2_1;OrgApacheHttpAuthClassLibrary">
		<owl:equivalentClass rdf:resource="&android-1_6;OrgApacheHttpAuthClassLibrary"/>
		<rdfs:subClassOf rdf:resource="&java;JavaClassLibrary"/>
		<rdfs:comment xml:lang="en">JavaLibrary implementing the org.apache.http.auth package for Android 2.1</rdfs:comment>
		<rdfs:comment xml:lang="OWLManchester">platform:implementsInterface some OrgApacheHttpAuthAPI</rdfs:comment>
	</owl:Class>
	<owl:Class rdf:about="&android-2_1;OrgApacheHttpAuthParamsClassLibrary">
		<owl:equivalentClass rdf:resource="&android-1_6;OrgApacheHttpAuthParamsClassLibrary"/>
		<rdfs:subClassOf rdf:resource="&java;JavaClassLibrary"/>
		<rdfs:comment xml:lang="en">JavaLibrary implementing the org.apache.http.auth.params package for Android 2.1</rdfs:comment>
		<rdfs:comment xml:lang="OWLManchester">platform:implementsInterface some OrgApacheHttpAuthParamsAPI</rdfs:comment>
	</owl:Class>
	<owl:Class rdf:about="&android-2_1;OrgApacheHttpClientClassLibrary">
		<owl:equivalentClass rdf:resource="&android-1_6;OrgApacheHttpClientClassLibrary"/>
		<rdfs:subClassOf rdf:resource="&java;JavaClassLibrary"/>
		<rdfs:comment xml:lang="en">JavaLibrary implementing the org.apache.http.client package for Android 2.1</rdfs:comment>
		<rdfs:comment xml:lang="OWLManchester">platform:implementsInterface some OrgApacheHttpClientAPI</rdfs:comment>
	</owl:Class>
	<owl:Class rdf:about="&android-2_1;OrgApacheHttpClientMethodsClassLibrary">
		<owl:equivalentClass rdf:resource="&android-1_6;OrgApacheHttpClientMethodsClassLibrary"/>
		<rdfs:subClassOf rdf:resource="&java;JavaClassLibrary"/>
		<rdfs:comment xml:lang="en">JavaLibrary implementing the org.apache.http.client.methods package for Android 2.1</rdfs:comment>
		<rdfs:comment xml:lang="OWLManchester">platform:implementsInterface some OrgApacheHttpClientMethodsAPI</rdfs:comment>
	</owl:Class>
	<owl:Class rdf:about="&android-2_1;OrgApacheHttpClientEntityClassLibrary">
		<owl:equivalentClass rdf:resource="&android-1_6;OrgApacheHttpClientEntityClassLibrary"/>
		<rdfs:subClassOf rdf:resource="&java;JavaClassLibrary"/>
		<rdfs:comment xml:lang="en">JavaLibrary implementing the org.apache.http.client.entity package for Android 2.1</rdfs:comment>
		<rdfs:comment xml:lang="OWLManchester">platform:implementsInterface some OrgApacheHttpClientEntityAPI</rdfs:comment>
	</owl:Class>
	<owl:Class rdf:about="&android-2_1;OrgApacheHttpClientParamsClassLibrary">
		<owl:equivalentClass rdf:resource="&android-1_6;OrgApacheHttpClientParamsClassLibrary"/>
		<rdfs:subClassOf rdf:resource="&java;JavaClassLibrary"/>
		<rdfs:comment xml:lang="en">JavaLibrary implementing the org.apache.http.client.params package for Android 2.1</rdfs:comment>
		<rdfs:comment xml:lang="OWLManchester">platform:implementsInterface some OrgApacheHttpClientParamsAPI</rdfs:comment>
	</owl:Class>
	<owl:Class rdf:about="&android-2_1;OrgApacheHttpClientProtocolClassLibrary">
		<owl:equivalentClass rdf:resource="&android-1_6;OrgApacheHttpClientProtocolClassLibrary"/>
		<rdfs:subClassOf rdf:resource="&java;JavaClassLibrary"/>
		<rdfs:comment xml:lang="en">JavaLibrary implementing the org.apache.http.client.protocol package for Android 2.1</rdfs:comment>
		<rdfs:comment xml:lang="OWLManchester">platform:implementsInterface some OrgApacheHttpClientProtocolAPI</rdfs:comment>
	</owl:Class>
	<owl:Class rdf:about="&android-2_1;OrgApacheHttpClientUtilsClassLibrary">
		<owl:equivalentClass rdf:resource="&android-1_6;OrgApacheHttpClientUtilsClassLibrary"/>
		<rdfs:subClassOf rdf:resource="&java;JavaClassLibrary"/>
		<rdfs:comment xml:lang="en">JavaLibrary implementing the org.apache.http.client.utils package for Android 2.1</rdfs:comment>
		<rdfs:comment xml:lang="OWLManchester">platform:implementsInterface some OrgApacheHttpClientUtilsAPI</rdfs:comment>
	</owl:Class>
	<owl:Class rdf:about="&android-2_1;OrgApacheHttpCookieClassLibrary">
		<owl:equivalentClass rdf:resource="&android-1_6;OrgApacheHttpCookieClassLibrary"/>
		<rdfs:subClassOf rdf:resource="&java;JavaClassLibrary"/>
		<rdfs:comment xml:lang="en">JavaLibrary implementing the org.apache.http.cookie package for Android 2.1</rdfs:comment>
		<rdfs:comment xml:lang="OWLManchester">platform:implementsInterface some OrgApacheHttpCookieAPI</rdfs:comment>
	</owl:Class>
	<owl:Class rdf:about="&android-2_1;OrgApacheHttpCookieParamsClassLibrary">
		<owl:equivalentClass rdf:resource="&android-1_6;OrgApacheHttpCookieParamsClassLibrary"/>
		<rdfs:subClassOf rdf:resource="&java;JavaClassLibrary"/>
		<rdfs:comment xml:lang="en">JavaLibrary implementing the org.apache.http.cookie.params package for Android 2.1</rdfs:comment>
		<rdfs:comment xml:lang="OWLManchester">platform:implementsInterface some OrgApacheHttpCookieParamsAPI</rdfs:comment>
	</owl:Class>
	<owl:Class rdf:about="&android-2_1;OrgApacheHttpConnClassLibrary">
		<owl:equivalentClass rdf:resource="&android-1_6;OrgApacheHttpConnClassLibrary"/>
		<rdfs:subClassOf rdf:resource="&java;JavaClassLibrary"/>
		<rdfs:comment xml:lang="en">JavaLibrary implementing the org.apache.http.conn package for Android 2.1</rdfs:comment>
		<rdfs:comment xml:lang="OWLManchester">platform:implementsInterface some OrgApacheHttpConnAPI</rdfs:comment>
	</owl:Class>
	<owl:Class rdf:about="&android-2_1;OrgApacheHttpConnParamsClassLibrary">
		<owl:equivalentClass rdf:resource="&android-1_6;OrgApacheHttpConnParamsClassLibrary"/>
		<rdfs:subClassOf rdf:resource="&java;JavaClassLibrary"/>
		<rdfs:comment xml:lang="en">JavaLibrary implementing the org.apache.http.conn.params package for Android 2.1</rdfs:comment>
		<rdfs:comment xml:lang="OWLManchester">platform:implementsInterface some OrgApacheHttpConnParamsAPI</rdfs:comment>
	</owl:Class>
	<owl:Class rdf:about="&android-2_1;OrgApacheHttpConnSchemeClassLibrary">
		<owl:equivalentClass rdf:resource="&android-1_6;OrgApacheHttpConnSchemeClassLibrary"/>
		<rdfs:subClassOf rdf:resource="&java;JavaClassLibrary"/>
		<rdfs:comment xml:lang="en">JavaLibrary implementing the org.apache.http.conn.scheme package for Android 2.1</rdfs:comment>
		<rdfs:comment xml:lang="OWLManchester">platform:implementsInterface some OrgApacheHttpConnSchemeAPI</rdfs:comment>
	</owl:Class>
	<owl:Class rdf:about="&android-2_1;OrgApacheHttpConnRoutingClassLibrary">
		<owl:equivalentClass rdf:resource="&android-1_6;OrgApacheHttpConnRoutingClassLibrary"/>
		<rdfs:subClassOf rdf:resource="&java;JavaClassLibrary"/>
		<rdfs:comment xml:lang="en">JavaLibrary implementing the org.apache.http.conn.routing package for Android 2.1</rdfs:comment>
		<rdfs:comment xml:lang="OWLManchester">platform:implementsInterface some OrgApacheHttpConnRoutingAPI</rdfs:comment>
	</owl:Class>
	<owl:Class rdf:about="&android-2_1;OrgApacheHttpConnSslClassLibrary">
		<owl:equivalentClass rdf:resource="&android-1_6;OrgApacheHttpConnSslClassLibrary"/>
		<rdfs:subClassOf rdf:resource="&java;JavaClassLibrary"/>
		<rdfs:comment xml:lang="en">JavaLibrary implementing the org.apache.http.conn.ssl package for Android 2.1</rdfs:comment>
		<rdfs:comment xml:lang="OWLManchester">platform:implementsInterface some OrgApacheHttpConnSslAPI</rdfs:comment>
	</owl:Class>
	<owl:Class rdf:about="&android-2_1;OrgApacheHttpConnUtilClassLibrary">
		<owl:equivalentClass rdf:resource="&android-1_6;OrgApacheHttpConnUtilClassLibrary"/>
		<rdfs:subClassOf rdf:resource="&java;JavaClassLibrary"/>
		<rdfs:comment xml:lang="en">JavaLibrary implementing the org.apache.http.conn.util package for Android 2.1</rdfs:comment>
		<rdfs:comment xml:lang="OWLManchester">platform:implementsInterface some OrgApacheHttpConnUtilAPI</rdfs:comment>
	</owl:Class>
	<owl:Class rdf:about="&android-2_1;OrgApacheHttpEntityClassLibrary">
		<owl:equivalentClass rdf:resource="&android-1_6;OrgApacheHttpEntityClassLibrary"/>
		<rdfs:subClassOf rdf:resource="&java;JavaClassLibrary"/>
		<rdfs:comment xml:lang="en">JavaLibrary implementing the org.apache.http.entity package for Android 2.1</rdfs:comment>
		<rdfs:comment xml:lang="OWLManchester">platform:implementsInterface some OrgApacheHttpEntityAPI</rdfs:comment>
	</owl:Class>
	<owl:Class rdf:about="&android-2_1;OrgApacheHttpMessageClassLibrary">
		<owl:equivalentClass rdf:resource="&android-1_6;OrgApacheHttpMessageClassLibrary"/>
		<rdfs:subClassOf rdf:resource="&java;JavaClassLibrary"/>
		<rdfs:comment xml:lang="en">JavaLibrary implementing the org.apache.http.message package for Android 2.1</rdfs:comment>
		<rdfs:comment xml:lang="OWLManchester">platform:implementsInterface some OrgApacheHttpMessageAPI</rdfs:comment>
	</owl:Class>
	<owl:Class rdf:about="&android-2_1;OrgApacheHttpImplClassLibrary">
		<owl:equivalentClass rdf:resource="&android-1_6;OrgApacheHttpImplClassLibrary"/>
		<rdfs:subClassOf rdf:resource="&java;JavaClassLibrary"/>
		<rdfs:comment xml:lang="en">JavaLibrary implementing the org.apache.http.impl package for Android 2.1</rdfs:comment>
		<rdfs:comment xml:lang="OWLManchester">platform:implementsInterface some OrgApacheHttpImplAPI</rdfs:comment>
	</owl:Class>
	<owl:Class rdf:about="&android-2_1;OrgApacheHttpImplEntityClassLibrary">
		<owl:equivalentClass rdf:resource="&android-1_6;OrgApacheHttpImplEntityClassLibrary"/>
		<rdfs:subClassOf rdf:resource="&java;JavaClassLibrary"/>
		<rdfs:comment xml:lang="en">JavaLibrary implementing the org.apache.http.impl.entity package for Android 2.1</rdfs:comment>
		<rdfs:comment xml:lang="OWLManchester">platform:implementsInterface some OrgApacheHttpImplEntityAPI</rdfs:comment>
	</owl:Class>
	<owl:Class rdf:about="&android-2_1;OrgApacheHttpImplAuthClassLibrary">
		<owl:equivalentClass rdf:resource="&android-1_6;OrgApacheHttpImplAuthClassLibrary"/>
		<rdfs:subClassOf rdf:resource="&java;JavaClassLibrary"/>
		<rdfs:comment xml:lang="en">JavaLibrary implementing the org.apache.http.impl.auth package for Android 2.1</rdfs:comment>
		<rdfs:comment xml:lang="OWLManchester">platform:implementsInterface some OrgApacheHttpImplAuthAPI</rdfs:comment>
	</owl:Class>
	<owl:Class rdf:about="&android-2_1;OrgApacheHttpImplClientClassLibrary">
		<owl:equivalentClass rdf:resource="&android-1_6;OrgApacheHttpImplClientClassLibrary"/>
		<rdfs:subClassOf rdf:resource="&java;JavaClassLibrary"/>
		<rdfs:comment xml:lang="en">JavaLibrary implementing the org.apache.http.impl.client package for Android 2.1</rdfs:comment>
		<rdfs:comment xml:lang="OWLManchester">platform:implementsInterface some OrgApacheHttpImplClientAPI</rdfs:comment>
	</owl:Class>
	<owl:Class rdf:about="&android-2_1;OrgApacheHttpImplConnClassLibrary">
		<owl:equivalentClass rdf:resource="&android-1_6;OrgApacheHttpImplConnClassLibrary"/>
		<rdfs:subClassOf rdf:resource="&java;JavaClassLibrary"/>
		<rdfs:comment xml:lang="en">JavaLibrary implementing the org.apache.http.impl.conn package for Android 2.1</rdfs:comment>
		<rdfs:comment xml:lang="OWLManchester">platform:implementsInterface some OrgApacheHttpImplConnAPI</rdfs:comment>
	</owl:Class>
	<owl:Class rdf:about="&android-2_1;OrgApacheHttpImplConnTsccmClassLibrary">
		<owl:equivalentClass rdf:resource="&android-1_6;OrgApacheHttpImplConnTsccmClassLibrary"/>
		<rdfs:subClassOf rdf:resource="&java;JavaClassLibrary"/>
		<rdfs:comment xml:lang="en">JavaLibrary implementing the org.apache.http.impl.conn.tsccm package for Android 2.1</rdfs:comment>
		<rdfs:comment xml:lang="OWLManchester">platform:implementsInterface some OrgApacheHttpImplConnTsccmAPI</rdfs:comment>
	</owl:Class>
	<owl:Class rdf:about="&android-2_1;OrgApacheHttpImplIoClassLibrary">
		<owl:equivalentClass rdf:resource="&android-1_6;OrgApacheHttpImplIoClassLibrary"/>
		<rdfs:subClassOf rdf:resource="&java;JavaClassLibrary"/>
		<rdfs:comment xml:lang="en">JavaLibrary implementing the org.apache.http.impl.io package for Android 2.1</rdfs:comment>
		<rdfs:comment xml:lang="OWLManchester">platform:implementsInterface some OrgApacheHttpImplIoAPI</rdfs:comment>
	</owl:Class>
	<owl:Class rdf:about="&android-2_1;OrgApacheHttpImplCookieClassLibrary">
		<owl:equivalentClass rdf:resource="&android-1_6;OrgApacheHttpImplCookieClassLibrary"/>
		<rdfs:subClassOf rdf:resource="&java;JavaClassLibrary"/>
		<rdfs:comment xml:lang="en">JavaLibrary implementing the org.apache.http.impl.cookie package for Android 2.1</rdfs:comment>
		<rdfs:comment xml:lang="OWLManchester">platform:implementsInterface some OrgApacheHttpImplCookieAPI</rdfs:comment>
	</owl:Class>
	<owl:Class rdf:about="&android-2_1;OrgApacheHttpIoClassLibrary">
		<owl:equivalentClass rdf:resource="&android-1_6;OrgApacheHttpIoClassLibrary"/>
		<rdfs:subClassOf rdf:resource="&java;JavaClassLibrary"/>
		<rdfs:comment xml:lang="en">JavaLibrary implementing the org.apache.http.io package for Android 2.1</rdfs:comment>
		<rdfs:comment xml:lang="OWLManchester">platform:implementsInterface some OrgApacheHttpIoAPI</rdfs:comment>
	</owl:Class>
	<owl:Class rdf:about="&android-2_1;OrgJsonClassLibrary">
		<owl:equivalentClass rdf:resource="&android-1_6;OrgJsonClassLibrary"/>
		<rdfs:subClassOf rdf:resource="&java;JavaClassLibrary"/>
		<rdfs:comment xml:lang="en">JavaLibrary implementing the org.json package for Android 2.1</rdfs:comment>
		<rdfs:comment xml:lang="OWLManchester">platform:implementsInterface some OrgJsonAPI</rdfs:comment>
	</owl:Class>
	<owl:Class rdf:about="&android-2_1;JavaxMicroeditionKhronosOpenglesClassLibrary">
		<owl:equivalentClass rdf:resource="&android-1_6;JavaxMicroeditionKhronosOpenglesClassLibrary"/>
		<rdfs:subClassOf rdf:resource="&java;JavaClassLibrary"/>
		<rdfs:comment xml:lang="en">JavaLibrary implementing the javax.microedition.khronos.opengles package for Android 2.1</rdfs:comment>
		<rdfs:comment xml:lang="OWLManchester">platform:implementsInterface some JavaxMicroeditionKhronosOpenglesAPI</rdfs:comment>
	</owl:Class>
	<owl:Class rdf:about="&android-2_1;JavaxMicroeditionKhronosEglClassLibrary">
		<owl:equivalentClass rdf:resource="&android-1_6;JavaxMicroeditionKhronosEglClassLibrary"/>
		<rdfs:subClassOf rdf:resource="&java;JavaClassLibrary"/>
		<rdfs:comment xml:lang="en">JavaLibrary implementing the javax.microedition.khronos.egl package for Android 2.1</rdfs:comment>
		<rdfs:comment xml:lang="OWLManchester">platform:implementsInterface some JavaxMicroeditionKhronosEglAPI</rdfs:comment>
	</owl:Class>
	<owl:Class rdf:about="&android-2_1;JavaxNetClassLibrary">
		<owl:equivalentClass rdf:resource="&java-se-6;JavaxNetClassLibrary"/>
		<owl:equivalentClass rdf:resource="&android-1_6;JavaxNetClassLibrary"/>
		<rdfs:subClassOf rdf:resource="&java;JavaClassLibrary"/>
		<rdfs:comment xml:lang="en">JavaLibrary implementing the javax.net package for Android 2.1</rdfs:comment>
		<rdfs:comment xml:lang="OWLManchester">platform:implementsInterface some JavaxNetAPI</rdfs:comment>
	</owl:Class>
	<owl:Class rdf:about="&android-2_1;JavaxNetSslClassLibrary">
		<owl:equivalentClass rdf:resource="&android-1_6;JavaxNetSslClassLibrary"/>
		<rdfs:subClassOf rdf:resource="&java;JavaClassLibrary"/>
		<rdfs:comment xml:lang="en">JavaLibrary implementing the javax.net.ssl package for Android 2.1</rdfs:comment>
		<rdfs:comment xml:lang="OWLManchester">platform:implementsInterface some JavaxNetSslAPI</rdfs:comment>
	</owl:Class>
	<owl:Class rdf:about="&android-2_1;JavaxSecurityAuthClassLibrary">
		<owl:equivalentClass rdf:resource="&android-1_6;JavaxSecurityAuthClassLibrary"/>
		<rdfs:subClassOf rdf:resource="&java;JavaClassLibrary"/>
		<rdfs:comment xml:lang="en">JavaLibrary implementing the javax.security.auth package for Android 2.1</rdfs:comment>
		<rdfs:comment xml:lang="OWLManchester">platform:implementsInterface some JavaxSecurityAuthAPI</rdfs:comment>
	</owl:Class>
	<owl:Class rdf:about="&android-2_1;JavaxSecurityAuthCallbackClassLibrary">
		<owl:equivalentClass rdf:resource="&android-1_6;JavaxSecurityAuthCallbackClassLibrary"/>
		<rdfs:subClassOf rdf:resource="&java;JavaClassLibrary"/>
		<rdfs:comment xml:lang="en">JavaLibrary implementing the javax.security.auth.callback package for Android 2.1</rdfs:comment>
		<rdfs:comment xml:lang="OWLManchester">platform:implementsInterface some JavaxSecurityAuthCallbackAPI</rdfs:comment>
	</owl:Class>
	<owl:Class rdf:about="&android-2_1;JavaxSecurityAuthX500ClassLibrary">
		<owl:equivalentClass rdf:resource="&android-1_6;JavaxSecurityAuthX500ClassLibrary"/>
		<rdfs:subClassOf rdf:resource="&java;JavaClassLibrary"/>
		<rdfs:comment xml:lang="en">JavaLibrary implementing the javax.security.auth.x500 package for Android 2.1</rdfs:comment>
		<rdfs:comment xml:lang="OWLManchester">platform:implementsInterface some JavaxSecurityAuthX500API</rdfs:comment>
	</owl:Class>
	<owl:Class rdf:about="&android-2_1;JavaxSecurityAuthLoginClassLibrary">
		<owl:equivalentClass rdf:resource="&android-1_6;JavaxSecurityAuthLoginClassLibrary"/>
		<rdfs:subClassOf rdf:resource="&java;JavaClassLibrary"/>
		<rdfs:comment xml:lang="en">JavaLibrary implementing the javax.security.auth.login package for Android 2.1</rdfs:comment>
		<rdfs:comment xml:lang="OWLManchester">platform:implementsInterface some JavaxSecurityAuthLoginAPI</rdfs:comment>
	</owl:Class>
	<owl:Class rdf:about="&android-2_1;JavaxSecurityCertClassLibrary">
		<owl:equivalentClass rdf:resource="&java-se-6;JavaxSecurityCertClassLibrary"/>
		<owl:equivalentClass rdf:resource="&android-1_6;JavaxSecurityCertClassLibrary"/>
		<rdfs:subClassOf rdf:resource="&java;JavaClassLibrary"/>
		<rdfs:comment xml:lang="en">JavaLibrary implementing the javax.security.cert package for Android 2.1</rdfs:comment>
		<rdfs:comment xml:lang="OWLManchester">platform:implementsInterface some JavaxSecurityCertAPI</rdfs:comment>
	</owl:Class>
	<owl:Class rdf:about="&android-2_1;JavaxCryptoClassLibrary">
		<owl:equivalentClass rdf:resource="&java-se-6;JavaxCryptoClassLibrary"/>
		<owl:equivalentClass rdf:resource="&android-1_6;JavaxCryptoClassLibrary"/>
		<rdfs:subClassOf rdf:resource="&java;JavaClassLibrary"/>
		<rdfs:comment xml:lang="en">JavaLibrary implementing the javax.crypto package for Android 2.1</rdfs:comment>
		<rdfs:comment xml:lang="OWLManchester">platform:implementsInterface some JavaxCryptoAPI</rdfs:comment>
	</owl:Class>
	<owl:Class rdf:about="&android-2_1;JavaxCryptoInterfacesClassLibrary">
		<owl:equivalentClass rdf:resource="&java-se-6;JavaxCryptoInterfacesClassLibrary"/>
		<owl:equivalentClass rdf:resource="&android-1_6;JavaxCryptoInterfacesClassLibrary"/>
		<rdfs:subClassOf rdf:resource="&java;JavaClassLibrary"/>
		<rdfs:comment xml:lang="en">JavaLibrary implementing the javax.crypto.interfaces package for Android 2.1</rdfs:comment>
		<rdfs:comment xml:lang="OWLManchester">platform:implementsInterface some JavaxCryptoInterfacesAPI</rdfs:comment>
	</owl:Class>
	<owl:Class rdf:about="&android-2_1;JavaxCryptoSpecClassLibrary">
		<owl:equivalentClass rdf:resource="&java-se-6;JavaxCryptoSpecClassLibrary"/>
		<owl:equivalentClass rdf:resource="&android-1_6;JavaxCryptoSpecClassLibrary"/>
		<rdfs:subClassOf rdf:resource="&java;JavaClassLibrary"/>
		<rdfs:comment xml:lang="en">JavaLibrary implementing the javax.crypto.spec package for Android 2.1</rdfs:comment>
		<rdfs:comment xml:lang="OWLManchester">platform:implementsInterface some JavaxCryptoSpecAPI</rdfs:comment>
	</owl:Class>
	<owl:Class rdf:about="&android-2_1;JavaxSqlClassLibrary">
		<owl:equivalentClass rdf:resource="&android-1_6;JavaxSqlClassLibrary"/>
		<rdfs:subClassOf rdf:resource="&java;JavaClassLibrary"/>
		<rdfs:comment xml:lang="en">JavaLibrary implementing the javax.sql package for Android 2.1</rdfs:comment>
		<rdfs:comment xml:lang="OWLManchester">platform:implementsInterface some JavaxSqlAPI</rdfs:comment>
	</owl:Class>
	<owl:Class rdf:about="&android-2_1;JavaxXmlClassLibrary">
		<owl:equivalentClass rdf:resource="&android-1_6;JavaxXmlClassLibrary"/>
		<rdfs:subClassOf rdf:resource="&java-se-6;JavaxXmlClassLibrary"/>
		<rdfs:comment xml:lang="en">JavaLibrary implementing the javax.xml package for Android 2.1</rdfs:comment>
		<rdfs:comment xml:lang="OWLManchester">platform:implementsInterface some JavaxXmlAPI</rdfs:comment>
	</owl:Class>
	<owl:Class rdf:about="&android-2_1;JavaxXmlParsersClassLibrary">
		<owl:equivalentClass rdf:resource="&android-1_6;JavaxXmlParsersClassLibrary"/>
		<rdfs:subClassOf rdf:resource="&java;JavaClassLibrary"/>
		<rdfs:comment xml:lang="en">JavaLibrary implementing the javax.xml.parsers package for Android 2.1</rdfs:comment>
		<rdfs:comment xml:lang="OWLManchester">platform:implementsInterface some JavaxXmlParsersAPI</rdfs:comment>
	</owl:Class>
	<owl:Class rdf:about="&android-2_1;JunitFrameworkClassLibrary">
		<owl:equivalentClass rdf:resource="&android-1_6;JunitFrameworkClassLibrary"/>
		<rdfs:subClassOf rdf:resource="&java;JavaClassLibrary"/>
		<rdfs:comment xml:lang="en">JavaLibrary implementing the junit.framework package for Android 2.1</rdfs:comment>
		<rdfs:comment xml:lang="OWLManchester">platform:implementsInterface some JunitFrameworkAPI</rdfs:comment>
	</owl:Class>
	<owl:Class rdf:about="&android-2_1;JunitRunnerClassLibrary">
		<owl:equivalentClass rdf:resource="&android-1_6;JunitRunnerClassLibrary"/>
		<rdfs:subClassOf rdf:resource="&java;JavaClassLibrary"/>
		<rdfs:comment xml:lang="en">JavaLibrary implementing the junit.runner package for Android 2.1</rdfs:comment>
		<rdfs:comment xml:lang="OWLManchester">platform:implementsInterface some JunitRunnerAPI</rdfs:comment>
	</owl:Class>
	<owl:Class rdf:about="&android-2_1;DalvikAnnotationClassLibrary">
		<owl:equivalentClass rdf:resource="&android-1_6;DalvikAnnotationClassLibrary"/>
		<rdfs:subClassOf rdf:resource="&java;JavaClassLibrary"/>
		<rdfs:comment xml:lang="en">JavaLibrary implementing the dalvik.annotation package for Android 2.1</rdfs:comment>
		<rdfs:comment xml:lang="OWLManchester">platform:implementsInterface some DalvikAnnotationAPI</rdfs:comment>
	</owl:Class>
	<owl:Class rdf:about="&android-2_1;DalvikBytecodeClassLibrary">
		<owl:equivalentClass rdf:resource="&android-1_6;DalvikBytecodeClassLibrary"/>
		<rdfs:subClassOf rdf:resource="&java;JavaClassLibrary"/>
		<rdfs:comment xml:lang="en">JavaLibrary implementing the dalvik.bytecode package for Android 2.1</rdfs:comment>
		<rdfs:comment xml:lang="OWLManchester">platform:implementsInterface some DalvikBytecodeAPI</rdfs:comment>
	</owl:Class>
	<owl:Class rdf:about="&android-2_1;DalvikSystemClassLibrary">
		<owl:equivalentClass rdf:resource="&android-1_6;DalvikSystemClassLibrary"/>
		<rdfs:subClassOf rdf:resource="&java;JavaClassLibrary"/>
		<rdfs:comment xml:lang="en">JavaLibrary implementing the dalvik.system package for Android 2.1</rdfs:comment>
		<rdfs:comment xml:lang="OWLManchester">platform:implementsInterface some DalvikSystemAPI</rdfs:comment>
	</owl:Class>
</rdf:RDF>
