<?xml version="1.0" encoding="ISO-8859-1"?>
<!DOCTYPE rdf:RDF [
	<!ENTITY j2me-midp-1_0 "http://ssel.vub.ac.be/platformkit/j2me-midp-1_0#">
	<!ENTITY units "http://localhost/~dennis/Units.owl#">
	<!ENTITY platform "http://localhost/~dennis/Platform.owl#">
	<!ENTITY java "http://localhost/~dennis/Java.owl#">
	<!ENTITY j2me-pp-1_0 "http://ssel.vub.ac.be/platformkit/j2me-pp-1_0#">
	<!ENTITY xsd "http://www.w3.org/2001/XMLSchema#">
	<!ENTITY owl "http://www.w3.org/2002/07/owl#">
	<!ENTITY rdfs "http://www.w3.org/2000/01/rdf-schema#">
	<!ENTITY rdf "http://www.w3.org/1999/02/22-rdf-syntax-ns#">
]>
<rdf:RDF
	 xmlns:j2me-midp-1_0="&j2me-midp-1_0;"
	 xmlns:units="&units;"
	 xmlns:platform="&platform;"
	 xmlns:java="&java;"
	 xmlns:j2me-pp-1_0="&j2me-pp-1_0;"
	 xmlns:xsd="&xsd;"
	 xmlns:owl="&owl;"
	 xmlns:rdfs="&rdfs;"
	 xmlns:rdf="&rdf;"
>

	<owl:Ontology rdf:about="http://ssel.vub.ac.be/platformkit/j2me-pp-1_0#">
		<owl:imports rdf:resource="http://ssel.vub.ac.be/platformkit/j2me-midp-1_0#"/>
		<owl:imports rdf:resource="http://localhost/~dennis/Platform.owl"/>
		<owl:imports rdf:resource="http://localhost/~dennis/Java.owl"/>
		<rdfs:comment xml:lang="en">Generated by $Id: UML2ToPackageAPIOntology.atl 6744 2007-05-25 09:44:28Z dwagelaa $</rdfs:comment>
		<rdfs:label xml:lang="en">j2me-pp-1_0</rdfs:label>
	</owl:Ontology>
	<owl:Class rdf:about="&j2me-pp-1_0;J2me-pp-1_0ClassLibrary">
		<rdfs:subClassOf rdf:resource="&j2me-pp-1_0;JavaLangLibrary"/>
		<rdfs:subClassOf rdf:resource="&j2me-pp-1_0;JavaAwtPeerLibrary"/>
		<rdfs:subClassOf rdf:resource="&j2me-pp-1_0;JavaSecurityInterfacesLibrary"/>
		<rdfs:subClassOf rdf:resource="&j2me-pp-1_0;JavaAwtLibrary"/>
		<rdfs:subClassOf rdf:resource="&j2me-pp-1_0;JavaSecurityAclLibrary"/>
		<rdfs:subClassOf rdf:resource="&j2me-pp-1_0;JavaLangRefLibrary"/>
		<rdfs:subClassOf rdf:resource="&j2me-pp-1_0;JavaAwtEventLibrary"/>
		<rdfs:subClassOf rdf:resource="&j2me-pp-1_0;JavaSecurityCertLibrary"/>
		<rdfs:subClassOf rdf:resource="&j2me-pp-1_0;JavaAwtColorLibrary"/>
		<rdfs:subClassOf rdf:resource="&j2me-pp-1_0;JavaRmiRegistryLibrary"/>
		<rdfs:subClassOf rdf:resource="&j2me-pp-1_0;JavaBeansLibrary"/>
		<rdfs:subClassOf rdf:resource="&j2me-pp-1_0;JavaAppletLibrary"/>
		<rdfs:subClassOf rdf:resource="&j2me-pp-1_0;JavaxMicroeditionXletIxcLibrary"/>
		<rdfs:subClassOf rdf:resource="&j2me-pp-1_0;JavaTextResourcesLibrary"/>
		<rdfs:subClassOf rdf:resource="&j2me-pp-1_0;JavaMathLibrary"/>
		<rdfs:subClassOf rdf:resource="&j2me-pp-1_0;JavaIoLibrary"/>
		<rdfs:subClassOf rdf:resource="&j2me-pp-1_0;JavaUtilJarLibrary"/>
		<rdfs:subClassOf rdf:resource="&j2me-pp-1_0;JavaRmiLibrary"/>
		<rdfs:subClassOf rdf:resource="&j2me-pp-1_0;JavaNetLibrary"/>
		<rdfs:subClassOf rdf:resource="&j2me-pp-1_0;JavaLangReflectLibrary"/>
		<rdfs:subClassOf rdf:resource="&j2me-pp-1_0;JavaAwtDatatransferLibrary"/>
		<rdfs:subClassOf rdf:resource="&j2me-pp-1_0;JavaTextLibrary"/>
		<rdfs:subClassOf rdf:resource="&j2me-pp-1_0;JavaxMicroeditionIoLibrary"/>
		<rdfs:subClassOf rdf:resource="&j2me-pp-1_0;JavaSecuritySpecLibrary"/>
		<rdfs:subClassOf rdf:resource="&j2me-pp-1_0;JavaUtilLibrary"/>
		<rdfs:subClassOf rdf:resource="&j2me-pp-1_0;JavaSecurityLibrary"/>
		<rdfs:subClassOf rdf:resource="&j2me-pp-1_0;JavaxMicroeditionXletLibrary"/>
		<rdfs:subClassOf rdf:resource="&j2me-pp-1_0;JavaUtilZipLibrary"/>
		<rdfs:subClassOf rdf:resource="&j2me-pp-1_0;JavaAwtImageLibrary"/>
		<rdfs:comment xml:lang="en">JavaLibrary implementing the entire API for j2me-pp-1_0</rdfs:comment>
	</owl:Class>
	<owl:Class rdf:about="&j2me-pp-1_0;J2me-pp-1_0">
		<rdfs:subClassOf rdf:resource="&java;JRE"/>
		<rdfs:subClassOf>
			<owl:Restriction>
				<owl:onProperty rdf:resource="&java;providesBuiltinJavaLibrary"/>
				<owl:someValuesFrom rdf:resource="&j2me-pp-1_0;J2me-pp-1_0ClassLibrary"/>
			</owl:Restriction>
		</rdfs:subClassOf>
		<rdfs:comment xml:lang="en">j2me-pp-1_0 Java Runtime Environment</rdfs:comment>
	</owl:Class>
	<owl:Class rdf:about="&j2me-pp-1_0;JavaLangLibrary">
		<rdfs:subClassOf rdf:resource="&java;JavaLibrary"/>
		<rdfs:seeAlso rdf:resource="&j2me-pp-1_0;JavaIoLibrary"/>
		<rdfs:seeAlso rdf:resource="&j2me-pp-1_0;JavaNetLibrary"/>
		<rdfs:seeAlso rdf:resource="&j2me-pp-1_0;JavaLangReflectLibrary"/>
		<rdfs:seeAlso rdf:resource="&j2me-pp-1_0;JavaSecurityLibrary"/>
		<rdfs:seeAlso rdf:resource="&j2me-pp-1_0;JavaUtilLibrary"/>
		<rdfs:comment xml:lang="en">JavaLibrary implementing the java.lang package for j2me-pp-1_0</rdfs:comment>
	</owl:Class>
	<owl:Class rdf:about="&j2me-pp-1_0;JavaAwtPeerLibrary">
		<rdfs:subClassOf rdf:resource="&java;JavaLibrary"/>
		<rdfs:seeAlso rdf:resource="&j2me-pp-1_0;JavaLangLibrary"/>
		<rdfs:seeAlso rdf:resource="&j2me-pp-1_0;JavaAwtLibrary"/>
		<rdfs:seeAlso rdf:resource="&j2me-pp-1_0;JavaAwtEventLibrary"/>
		<rdfs:seeAlso rdf:resource="&j2me-pp-1_0;JavaIoLibrary"/>
		<rdfs:seeAlso rdf:resource="&j2me-pp-1_0;JavaAwtImageLibrary"/>
		<rdfs:comment xml:lang="en">JavaLibrary implementing the java.awt.peer package for j2me-pp-1_0</rdfs:comment>
	</owl:Class>
	<owl:Class rdf:about="&j2me-pp-1_0;JavaSecurityInterfacesLibrary">
		<rdfs:subClassOf rdf:resource="&java;JavaLibrary"/>
		<rdfs:seeAlso rdf:resource="&j2me-pp-1_0;JavaMathLibrary"/>
		<rdfs:seeAlso rdf:resource="&j2me-pp-1_0;JavaSecurityLibrary"/>
		<rdfs:comment xml:lang="en">JavaLibrary implementing the java.security.interfaces package for j2me-pp-1_0</rdfs:comment>
	</owl:Class>
	<owl:Class rdf:about="&j2me-pp-1_0;JavaAwtLibrary">
		<rdfs:subClassOf rdf:resource="&java;JavaLibrary"/>
		<rdfs:seeAlso rdf:resource="&j2me-pp-1_0;JavaLangLibrary"/>
		<rdfs:seeAlso rdf:resource="&j2me-pp-1_0;JavaAwtPeerLibrary"/>
		<rdfs:seeAlso rdf:resource="&j2me-pp-1_0;JavaAwtEventLibrary"/>
		<rdfs:seeAlso rdf:resource="&j2me-pp-1_0;JavaSecurityLibrary"/>
		<rdfs:seeAlso rdf:resource="&j2me-pp-1_0;JavaAwtImageLibrary"/>
		<rdfs:seeAlso rdf:resource="&j2me-pp-1_0;JavaAwtColorLibrary"/>
		<rdfs:seeAlso rdf:resource="&j2me-pp-1_0;JavaBeansLibrary"/>
		<rdfs:seeAlso rdf:resource="&j2me-pp-1_0;JavaIoLibrary"/>
		<rdfs:seeAlso rdf:resource="&j2me-pp-1_0;JavaNetLibrary"/>
		<rdfs:seeAlso rdf:resource="&j2me-pp-1_0;JavaAwtDatatransferLibrary"/>
		<rdfs:seeAlso rdf:resource="&j2me-pp-1_0;JavaTextLibrary"/>
		<rdfs:seeAlso rdf:resource="&j2me-pp-1_0;JavaUtilLibrary"/>
		<rdfs:comment xml:lang="en">JavaLibrary implementing the java.awt package for j2me-pp-1_0</rdfs:comment>
	</owl:Class>
	<owl:Class rdf:about="&j2me-pp-1_0;JavaSecurityAclLibrary">
		<rdfs:subClassOf rdf:resource="&java;JavaLibrary"/>
		<rdfs:seeAlso rdf:resource="&j2me-pp-1_0;JavaLangLibrary"/>
		<rdfs:seeAlso rdf:resource="&j2me-pp-1_0;JavaSecurityLibrary"/>
		<rdfs:seeAlso rdf:resource="&j2me-pp-1_0;JavaUtilLibrary"/>
		<rdfs:comment xml:lang="en">JavaLibrary implementing the java.security.acl package for j2me-pp-1_0</rdfs:comment>
	</owl:Class>
	<owl:Class rdf:about="&j2me-pp-1_0;JavaLangRefLibrary">
		<rdfs:subClassOf rdf:resource="&java;JavaLibrary"/>
		<rdfs:seeAlso rdf:resource="&j2me-pp-1_0;JavaLangLibrary"/>
		<rdfs:comment xml:lang="en">JavaLibrary implementing the java.lang.ref package for j2me-pp-1_0</rdfs:comment>
	</owl:Class>
	<owl:Class rdf:about="&j2me-pp-1_0;JavaAwtEventLibrary">
		<rdfs:subClassOf rdf:resource="&java;JavaLibrary"/>
		<rdfs:seeAlso rdf:resource="&j2me-pp-1_0;JavaLangLibrary"/>
		<rdfs:seeAlso rdf:resource="&j2me-pp-1_0;JavaAwtLibrary"/>
		<rdfs:seeAlso rdf:resource="&j2me-pp-1_0;JavaTextLibrary"/>
		<rdfs:seeAlso rdf:resource="&j2me-pp-1_0;JavaUtilLibrary"/>
		<rdfs:comment xml:lang="en">JavaLibrary implementing the java.awt.event package for j2me-pp-1_0</rdfs:comment>
	</owl:Class>
	<owl:Class rdf:about="&j2me-pp-1_0;JavaSecurityCertLibrary">
		<rdfs:subClassOf rdf:resource="&java;JavaLibrary"/>
		<rdfs:seeAlso rdf:resource="&j2me-pp-1_0;JavaMathLibrary"/>
		<rdfs:seeAlso rdf:resource="&j2me-pp-1_0;JavaIoLibrary"/>
		<rdfs:seeAlso rdf:resource="&j2me-pp-1_0;JavaLangLibrary"/>
		<rdfs:seeAlso rdf:resource="&j2me-pp-1_0;JavaSecurityLibrary"/>
		<rdfs:seeAlso rdf:resource="&j2me-pp-1_0;JavaUtilLibrary"/>
		<rdfs:comment xml:lang="en">JavaLibrary implementing the java.security.cert package for j2me-pp-1_0</rdfs:comment>
	</owl:Class>
	<owl:Class rdf:about="&j2me-pp-1_0;JavaAwtColorLibrary">
		<rdfs:subClassOf rdf:resource="&java;JavaLibrary"/>
		<rdfs:seeAlso rdf:resource="&j2me-pp-1_0;JavaIoLibrary"/>
		<rdfs:seeAlso rdf:resource="&j2me-pp-1_0;JavaLangLibrary"/>
		<rdfs:comment xml:lang="en">JavaLibrary implementing the java.awt.color package for j2me-pp-1_0</rdfs:comment>
	</owl:Class>
	<owl:Class rdf:about="&j2me-pp-1_0;JavaRmiRegistryLibrary">
		<rdfs:subClassOf rdf:resource="&java;JavaLibrary"/>
		<rdfs:seeAlso rdf:resource="&j2me-pp-1_0;JavaRmiLibrary"/>
		<rdfs:seeAlso rdf:resource="&j2me-pp-1_0;JavaLangLibrary"/>
		<rdfs:comment xml:lang="en">JavaLibrary implementing the java.rmi.registry package for j2me-pp-1_0</rdfs:comment>
	</owl:Class>
	<owl:Class rdf:about="&j2me-pp-1_0;JavaBeansLibrary">
		<rdfs:subClassOf rdf:resource="&java;JavaLibrary"/>
		<rdfs:seeAlso rdf:resource="&j2me-pp-1_0;JavaIoLibrary"/>
		<rdfs:seeAlso rdf:resource="&j2me-pp-1_0;JavaLangLibrary"/>
		<rdfs:seeAlso rdf:resource="&j2me-pp-1_0;JavaLangReflectLibrary"/>
		<rdfs:seeAlso rdf:resource="&j2me-pp-1_0;JavaAwtLibrary"/>
		<rdfs:seeAlso rdf:resource="&j2me-pp-1_0;JavaUtilLibrary"/>
		<rdfs:seeAlso rdf:resource="&j2me-pp-1_0;JavaAppletLibrary"/>
		<rdfs:comment xml:lang="en">JavaLibrary implementing the java.beans package for j2me-pp-1_0</rdfs:comment>
	</owl:Class>
	<owl:Class rdf:about="&j2me-pp-1_0;JavaAppletLibrary">
		<rdfs:subClassOf rdf:resource="&java;JavaLibrary"/>
		<rdfs:seeAlso rdf:resource="&j2me-pp-1_0;JavaLangLibrary"/>
		<rdfs:seeAlso rdf:resource="&j2me-pp-1_0;JavaNetLibrary"/>
		<rdfs:seeAlso rdf:resource="&j2me-pp-1_0;JavaUtilLibrary"/>
		<rdfs:seeAlso rdf:resource="&j2me-pp-1_0;JavaAwtLibrary"/>
		<rdfs:comment xml:lang="en">JavaLibrary implementing the java.applet package for j2me-pp-1_0</rdfs:comment>
	</owl:Class>
	<owl:Class rdf:about="&j2me-pp-1_0;JavaxMicroeditionXletIxcLibrary">
		<rdfs:subClassOf rdf:resource="&java;JavaLibrary"/>
		<rdfs:seeAlso rdf:resource="&j2me-pp-1_0;JavaRmiLibrary"/>
		<rdfs:seeAlso rdf:resource="&j2me-pp-1_0;JavaLangLibrary"/>
		<rdfs:seeAlso rdf:resource="&j2me-pp-1_0;JavaRmiRegistryLibrary"/>
		<rdfs:seeAlso rdf:resource="&j2me-pp-1_0;JavaxMicroeditionXletLibrary"/>
		<rdfs:comment xml:lang="en">JavaLibrary implementing the javax.microedition.xlet.ixc package for j2me-pp-1_0</rdfs:comment>
	</owl:Class>
	<owl:Class rdf:about="&j2me-pp-1_0;JavaTextResourcesLibrary">
		<rdfs:subClassOf rdf:resource="&java;JavaLibrary"/>
		<rdfs:seeAlso rdf:resource="&j2me-pp-1_0;JavaLangLibrary"/>
		<rdfs:seeAlso rdf:resource="&j2me-pp-1_0;JavaUtilLibrary"/>
		<rdfs:comment xml:lang="en">JavaLibrary implementing the java.text.resources package for j2me-pp-1_0</rdfs:comment>
	</owl:Class>
	<owl:Class rdf:about="&j2me-pp-1_0;JavaMathLibrary">
		<rdfs:subClassOf rdf:resource="&java;JavaLibrary"/>
		<rdfs:seeAlso rdf:resource="&j2me-pp-1_0;JavaLangLibrary"/>
		<rdfs:seeAlso rdf:resource="&j2me-pp-1_0;JavaUtilLibrary"/>
		<rdfs:comment xml:lang="en">JavaLibrary implementing the java.math package for j2me-pp-1_0</rdfs:comment>
	</owl:Class>
	<owl:Class rdf:about="&j2me-pp-1_0;JavaIoLibrary">
		<rdfs:subClassOf rdf:resource="&java;JavaLibrary"/>
		<rdfs:seeAlso rdf:resource="&j2me-pp-1_0;JavaLangLibrary"/>
		<rdfs:seeAlso rdf:resource="&j2me-pp-1_0;JavaNetLibrary"/>
		<rdfs:seeAlso rdf:resource="&j2me-pp-1_0;JavaUtilLibrary"/>
		<rdfs:seeAlso rdf:resource="&j2me-pp-1_0;JavaSecurityLibrary"/>
		<rdfs:comment xml:lang="en">JavaLibrary implementing the java.io package for j2me-pp-1_0</rdfs:comment>
	</owl:Class>
	<owl:Class rdf:about="&j2me-pp-1_0;JavaUtilJarLibrary">
		<rdfs:subClassOf rdf:resource="&java;JavaLibrary"/>
		<rdfs:seeAlso rdf:resource="&j2me-pp-1_0;JavaIoLibrary"/>
		<rdfs:seeAlso rdf:resource="&j2me-pp-1_0;JavaLangLibrary"/>
		<rdfs:seeAlso rdf:resource="&j2me-pp-1_0;JavaUtilLibrary"/>
		<rdfs:seeAlso rdf:resource="&j2me-pp-1_0;JavaUtilZipLibrary"/>
		<rdfs:comment xml:lang="en">JavaLibrary implementing the java.util.jar package for j2me-pp-1_0</rdfs:comment>
	</owl:Class>
	<owl:Class rdf:about="&j2me-pp-1_0;JavaRmiLibrary">
		<rdfs:subClassOf rdf:resource="&java;JavaLibrary"/>
		<rdfs:seeAlso rdf:resource="&j2me-pp-1_0;JavaIoLibrary"/>
		<rdfs:seeAlso rdf:resource="&j2me-pp-1_0;JavaLangLibrary"/>
		<rdfs:comment xml:lang="en">JavaLibrary implementing the java.rmi package for j2me-pp-1_0</rdfs:comment>
	</owl:Class>
	<owl:Class rdf:about="&j2me-pp-1_0;JavaNetLibrary">
		<rdfs:subClassOf rdf:resource="&java;JavaLibrary"/>
		<rdfs:seeAlso rdf:resource="&j2me-pp-1_0;JavaIoLibrary"/>
		<rdfs:seeAlso rdf:resource="&j2me-pp-1_0;JavaUtilJarLibrary"/>
		<rdfs:seeAlso rdf:resource="&j2me-pp-1_0;JavaLangLibrary"/>
		<rdfs:seeAlso rdf:resource="&j2me-pp-1_0;JavaUtilLibrary"/>
		<rdfs:seeAlso rdf:resource="&j2me-pp-1_0;JavaSecurityLibrary"/>
		<rdfs:comment xml:lang="en">JavaLibrary implementing the java.net package for j2me-pp-1_0</rdfs:comment>
	</owl:Class>
	<owl:Class rdf:about="&j2me-pp-1_0;JavaLangReflectLibrary">
		<rdfs:subClassOf rdf:resource="&java;JavaLibrary"/>
		<rdfs:seeAlso rdf:resource="&j2me-pp-1_0;JavaIoLibrary"/>
		<rdfs:seeAlso rdf:resource="&j2me-pp-1_0;JavaLangLibrary"/>
		<rdfs:seeAlso rdf:resource="&j2me-pp-1_0;JavaSecurityLibrary"/>
		<rdfs:comment xml:lang="en">JavaLibrary implementing the java.lang.reflect package for j2me-pp-1_0</rdfs:comment>
	</owl:Class>
	<owl:Class rdf:about="&j2me-pp-1_0;JavaAwtDatatransferLibrary">
		<rdfs:subClassOf rdf:resource="&java;JavaLibrary"/>
		<rdfs:seeAlso rdf:resource="&j2me-pp-1_0;JavaIoLibrary"/>
		<rdfs:seeAlso rdf:resource="&j2me-pp-1_0;JavaLangLibrary"/>
		<rdfs:seeAlso rdf:resource="&j2me-pp-1_0;JavaUtilLibrary"/>
		<rdfs:comment xml:lang="en">JavaLibrary implementing the java.awt.datatransfer package for j2me-pp-1_0</rdfs:comment>
	</owl:Class>
	<owl:Class rdf:about="&j2me-pp-1_0;JavaTextLibrary">
		<rdfs:subClassOf rdf:resource="&java;JavaLibrary"/>
		<rdfs:seeAlso rdf:resource="&j2me-pp-1_0;JavaIoLibrary"/>
		<rdfs:seeAlso rdf:resource="&j2me-pp-1_0;JavaLangLibrary"/>
		<rdfs:seeAlso rdf:resource="&j2me-pp-1_0;JavaUtilLibrary"/>
		<rdfs:comment xml:lang="en">JavaLibrary implementing the java.text package for j2me-pp-1_0</rdfs:comment>
	</owl:Class>
	<owl:Class rdf:about="&j2me-pp-1_0;JavaxMicroeditionIoLibrary">
		<rdfs:subClassOf rdf:resource="&java;JavaLibrary"/>
		<rdfs:seeAlso rdf:resource="&j2me-pp-1_0;JavaIoLibrary"/>
		<rdfs:seeAlso rdf:resource="&j2me-pp-1_0;JavaLangLibrary"/>
		<rdfs:comment xml:lang="en">JavaLibrary implementing the javax.microedition.io package for j2me-pp-1_0</rdfs:comment>
	</owl:Class>
	<owl:Class rdf:about="&j2me-pp-1_0;JavaSecuritySpecLibrary">
		<rdfs:subClassOf rdf:resource="&java;JavaLibrary"/>
		<rdfs:seeAlso rdf:resource="&j2me-pp-1_0;JavaMathLibrary"/>
		<rdfs:seeAlso rdf:resource="&j2me-pp-1_0;JavaLangLibrary"/>
		<rdfs:seeAlso rdf:resource="&j2me-pp-1_0;JavaSecurityInterfacesLibrary"/>
		<rdfs:seeAlso rdf:resource="&j2me-pp-1_0;JavaSecurityLibrary"/>
		<rdfs:comment xml:lang="en">JavaLibrary implementing the java.security.spec package for j2me-pp-1_0</rdfs:comment>
	</owl:Class>
	<owl:Class rdf:about="&j2me-pp-1_0;JavaUtilLibrary">
		<rdfs:subClassOf rdf:resource="&java;JavaLibrary"/>
		<rdfs:seeAlso rdf:resource="&j2me-pp-1_0;JavaIoLibrary"/>
		<rdfs:seeAlso rdf:resource="&j2me-pp-1_0;JavaLangLibrary"/>
		<rdfs:seeAlso rdf:resource="&j2me-pp-1_0;JavaSecurityLibrary"/>
		<rdfs:comment xml:lang="en">JavaLibrary implementing the java.util package for j2me-pp-1_0</rdfs:comment>
	</owl:Class>
	<owl:Class rdf:about="&j2me-pp-1_0;JavaSecurityLibrary">
		<rdfs:subClassOf rdf:resource="&java;JavaLibrary"/>
		<rdfs:seeAlso rdf:resource="&j2me-pp-1_0;JavaLangLibrary"/>
		<rdfs:seeAlso rdf:resource="&j2me-pp-1_0;JavaSecurityCertLibrary"/>
		<rdfs:seeAlso rdf:resource="&j2me-pp-1_0;JavaIoLibrary"/>
		<rdfs:seeAlso rdf:resource="&j2me-pp-1_0;JavaNetLibrary"/>
		<rdfs:seeAlso rdf:resource="&j2me-pp-1_0;JavaSecuritySpecLibrary"/>
		<rdfs:seeAlso rdf:resource="&j2me-pp-1_0;JavaUtilLibrary"/>
		<rdfs:comment xml:lang="en">JavaLibrary implementing the java.security package for j2me-pp-1_0</rdfs:comment>
	</owl:Class>
	<owl:Class rdf:about="&j2me-pp-1_0;JavaxMicroeditionXletLibrary">
		<rdfs:subClassOf rdf:resource="&java;JavaLibrary"/>
		<rdfs:seeAlso rdf:resource="&j2me-pp-1_0;JavaLangLibrary"/>
		<rdfs:seeAlso rdf:resource="&j2me-pp-1_0;JavaAwtLibrary"/>
		<rdfs:comment xml:lang="en">JavaLibrary implementing the javax.microedition.xlet package for j2me-pp-1_0</rdfs:comment>
	</owl:Class>
	<owl:Class rdf:about="&j2me-pp-1_0;JavaUtilZipLibrary">
		<rdfs:subClassOf rdf:resource="&java;JavaLibrary"/>
		<rdfs:seeAlso rdf:resource="&j2me-pp-1_0;JavaIoLibrary"/>
		<rdfs:seeAlso rdf:resource="&j2me-pp-1_0;JavaLangLibrary"/>
		<rdfs:seeAlso rdf:resource="&j2me-pp-1_0;JavaUtilLibrary"/>
		<rdfs:comment xml:lang="en">JavaLibrary implementing the java.util.zip package for j2me-pp-1_0</rdfs:comment>
	</owl:Class>
	<owl:Class rdf:about="&j2me-pp-1_0;JavaAwtImageLibrary">
		<rdfs:subClassOf rdf:resource="&java;JavaLibrary"/>
		<rdfs:seeAlso rdf:resource="&j2me-pp-1_0;JavaMathLibrary"/>
		<rdfs:seeAlso rdf:resource="&j2me-pp-1_0;JavaLangLibrary"/>
		<rdfs:seeAlso rdf:resource="&j2me-pp-1_0;JavaAwtLibrary"/>
		<rdfs:seeAlso rdf:resource="&j2me-pp-1_0;JavaAwtColorLibrary"/>
		<rdfs:seeAlso rdf:resource="&j2me-pp-1_0;JavaUtilLibrary"/>
		<rdfs:comment xml:lang="en">JavaLibrary implementing the java.awt.image package for j2me-pp-1_0</rdfs:comment>
	</owl:Class>
</rdf:RDF>
