<?xml version="1.0" encoding="ISO-8859-1"?>
<!DOCTYPE rdf:RDF [
	<!ENTITY platform "http://localhost/~dennis/Platform.owl#">
	<!ENTITY java "http://localhost/~dennis/Java.owl#">
	<!ENTITY xsd "http://www.w3.org/2001/XMLSchema#">
	<!ENTITY units "http://localhost/~dennis/Units.owl#">
	<!ENTITY j2se-1_4 "http://ssel.vub.ac.be/platformkit/j2se-1_4#">
	<!ENTITY j2se-1_5 "http://ssel.vub.ac.be/platformkit/j2se-1_5#">
	<!ENTITY rdf "http://www.w3.org/1999/02/22-rdf-syntax-ns#">
	<!ENTITY rdfs "http://www.w3.org/2000/01/rdf-schema#">
	<!ENTITY owl "http://www.w3.org/2002/07/owl#">
]>
<rdf:RDF
	 xmlns:platform="&platform;"
	 xmlns:java="&java;"
	 xmlns:xsd="&xsd;"
	 xmlns:units="&units;"
	 xmlns:j2se-1_4="&j2se-1_4;"
	 xmlns:j2se-1_5="&j2se-1_5;"
	 xmlns:rdf="&rdf;"
	 xmlns:rdfs="&rdfs;"
	 xmlns:owl="&owl;"
>

	<owl:Ontology rdf:about="http://ssel.vub.ac.be/platformkit/j2se-1_5#">
		<owl:imports rdf:resource="http://localhost/~dennis/Platform.owl"/>
		<owl:imports rdf:resource="http://localhost/~dennis/Java.owl"/>
		<owl:imports rdf:resource="http://ssel.vub.ac.be/platformkit/j2se-1_4#"/>
		<rdfs:comment xml:lang="en">Generated by $Id: UML2ToPackageAPIOntology.atl 6744 2007-05-25 09:44:28Z dwagelaa $</rdfs:comment>
		<rdfs:label xml:lang="en">j2se-1_5</rdfs:label>
	</owl:Ontology>
	<owl:Class rdf:about="&j2se-1_5;J2se-1_5ClassLibrary">
		<rdfs:subClassOf rdf:resource="&j2se-1_5;OrgOmgCORBAPortableLibrary"/>
		<rdfs:subClassOf rdf:resource="&j2se-1_5;JavaxSqlLibrary"/>
		<rdfs:subClassOf rdf:resource="&j2se-1_5;JavaAwtImageLibrary"/>
		<rdfs:subClassOf rdf:resource="&j2se-1_5;OrgIetfJgssLibrary"/>
		<rdfs:subClassOf rdf:resource="&j2se-1_5;OrgOmgCORBADynAnyPackageLibrary"/>
		<rdfs:subClassOf rdf:resource="&j2se-1_5;JavaAwtImLibrary"/>
		<rdfs:subClassOf rdf:resource="&j2se-1_5;JavaLangAnnotationLibrary"/>
		<rdfs:subClassOf rdf:resource="&j2se-1_5;OrgOmgIOPCodecFactoryPackageLibrary"/>
		<rdfs:subClassOf rdf:resource="&j2se-1_5;JavaxManagementOpenmbeanLibrary"/>
		<rdfs:subClassOf rdf:resource="&j2se-1_5;JavaBeansBeancontextLibrary"/>
		<rdfs:subClassOf rdf:resource="&j2se-1_5;JavaUtilZipLibrary"/>
		<rdfs:subClassOf rdf:resource="&j2se-1_5;JavaxSwingTextHtmlParserLibrary"/>
		<rdfs:subClassOf rdf:resource="&j2se-1_5;JavaAwtImSpiLibrary"/>
		<rdfs:subClassOf rdf:resource="&j2se-1_5;JavaxXmlTransformDomLibrary"/>
		<rdfs:subClassOf rdf:resource="&j2se-1_5;JavaSecuritySpecLibrary"/>
		<rdfs:subClassOf rdf:resource="&j2se-1_5;JavaUtilJarLibrary"/>
		<rdfs:subClassOf rdf:resource="&j2se-1_5;JavaSecurityLibrary"/>
		<rdfs:subClassOf rdf:resource="&j2se-1_5;JavaxImageioEventLibrary"/>
		<rdfs:subClassOf rdf:resource="&j2se-1_5;JavaxSwingPlafMultiLibrary"/>
		<rdfs:subClassOf rdf:resource="&j2se-1_5;JavaAwtPrintLibrary"/>
		<rdfs:subClassOf rdf:resource="&j2se-1_5;JavaxXmlTransformStreamLibrary"/>
		<rdfs:subClassOf rdf:resource="&j2se-1_5;JavaxNamingEventLibrary"/>
		<rdfs:subClassOf rdf:resource="&j2se-1_5;JavaxSecuritySaslLibrary"/>
		<rdfs:subClassOf rdf:resource="&j2se-1_5;OrgOmgIOPCodecPackageLibrary"/>
		<rdfs:subClassOf rdf:resource="&j2se-1_5;JavaNioCharsetSpiLibrary"/>
		<rdfs:subClassOf rdf:resource="&j2se-1_5;JavaxXmlTransformLibrary"/>
		<rdfs:subClassOf rdf:resource="&j2se-1_5;OrgOmgPortableInterceptorORBInitInfoPackageLibrary"/>
		<rdfs:subClassOf rdf:resource="&j2se-1_5;JavaLangRefLibrary"/>
		<rdfs:subClassOf rdf:resource="&j2se-1_5;JavaxSecurityAuthLibrary"/>
		<rdfs:subClassOf rdf:resource="&j2se-1_5;JavaxSqlRowsetSerialLibrary"/>
		<rdfs:subClassOf rdf:resource="&j2se-1_5;JavaRmiLibrary"/>
		<rdfs:subClassOf rdf:resource="&j2se-1_5;JavaxManagementRemoteLibrary"/>
		<rdfs:subClassOf rdf:resource="&j2se-1_5;JavaxManagementLibrary"/>
		<rdfs:subClassOf rdf:resource="&j2se-1_5;JavaAwtLibrary"/>
		<rdfs:subClassOf rdf:resource="&j2se-1_5;JavaxManagementModelmbeanLibrary"/>
		<rdfs:subClassOf rdf:resource="&j2se-1_5;JavaxSwingTextRtfLibrary"/>
		<rdfs:subClassOf rdf:resource="&j2se-1_5;JavaNioChannelsLibrary"/>
		<rdfs:subClassOf rdf:resource="&j2se-1_5;JavaUtilConcurrentLocksLibrary"/>
		<rdfs:subClassOf rdf:resource="&j2se-1_5;JavaRmiServerLibrary"/>
		<rdfs:subClassOf rdf:resource="&j2se-1_5;OrgW3cDomHtmlLibrary"/>
		<rdfs:subClassOf rdf:resource="&j2se-1_5;JavaxSwingColorchooserLibrary"/>
		<rdfs:subClassOf rdf:resource="&j2se-1_5;OrgOmgPortableServerPOAManagerPackageLibrary"/>
		<rdfs:subClassOf rdf:resource="&j2se-1_5;JavaxImageioStreamLibrary"/>
		<rdfs:subClassOf rdf:resource="&j2se-1_5;JavaxXmlDatatypeLibrary"/>
		<rdfs:subClassOf rdf:resource="&j2se-1_5;JavaxRmiSslLibrary"/>
		<rdfs:subClassOf rdf:resource="&j2se-1_5;JavaxManagementRelationLibrary"/>
		<rdfs:subClassOf rdf:resource="&j2se-1_5;JavaUtilRegexLibrary"/>
		<rdfs:subClassOf rdf:resource="&j2se-1_5;OrgOmgMessagingLibrary"/>
		<rdfs:subClassOf rdf:resource="&j2se-1_5;JavaxSwingPlafMetalLibrary"/>
		<rdfs:subClassOf rdf:resource="&j2se-1_5;OrgW3cDomStylesheetsLibrary"/>
		<rdfs:subClassOf rdf:resource="&j2se-1_5;JavaxImageioPluginsBmpLibrary"/>
		<rdfs:subClassOf rdf:resource="&j2se-1_5;OrgXmlSaxHelpersLibrary"/>
		<rdfs:subClassOf rdf:resource="&j2se-1_5;JavaxSecurityAuthX500Library"/>
		<rdfs:subClassOf rdf:resource="&j2se-1_5;OrgOmgIOPLibrary"/>
		<rdfs:subClassOf rdf:resource="&j2se-1_5;OrgOmgCORBA_2_3PortableLibrary"/>
		<rdfs:subClassOf rdf:resource="&j2se-1_5;JavaxNamingLibrary"/>
		<rdfs:subClassOf rdf:resource="&j2se-1_5;JavaUtilConcurrentAtomicLibrary"/>
		<rdfs:subClassOf rdf:resource="&j2se-1_5;OrgOmgCORBATypeCodePackageLibrary"/>
		<rdfs:subClassOf rdf:resource="&j2se-1_5;OrgW3cDomLsLibrary"/>
		<rdfs:subClassOf rdf:resource="&j2se-1_5;OrgOmgCORBALibrary"/>
		<rdfs:subClassOf rdf:resource="&j2se-1_5;JavaxSwingPlafBasicLibrary"/>
		<rdfs:subClassOf rdf:resource="&j2se-1_5;JavaxManagementTimerLibrary"/>
		<rdfs:subClassOf rdf:resource="&j2se-1_5;JavaSecurityAclLibrary"/>
		<rdfs:subClassOf rdf:resource="&j2se-1_5;JavaAwtFontLibrary"/>
		<rdfs:subClassOf rdf:resource="&j2se-1_5;OrgOmgDynamicLibrary"/>
		<rdfs:subClassOf rdf:resource="&j2se-1_5;JavaRmiActivationLibrary"/>
		<rdfs:subClassOf rdf:resource="&j2se-1_5;JavaAwtGeomLibrary"/>
		<rdfs:subClassOf rdf:resource="&j2se-1_5;JavaAwtImageRenderableLibrary"/>
		<rdfs:subClassOf rdf:resource="&j2se-1_5;JavaIoLibrary"/>
		<rdfs:subClassOf rdf:resource="&j2se-1_5;JavaAwtEventLibrary"/>
		<rdfs:subClassOf rdf:resource="&j2se-1_5;OrgOmgPortableServerPOAPackageLibrary"/>
		<rdfs:subClassOf rdf:resource="&j2se-1_5;JavaxRmiLibrary"/>
		<rdfs:subClassOf rdf:resource="&j2se-1_5;JavaAwtPeerLibrary"/>
		<rdfs:subClassOf rdf:resource="&j2se-1_5;OrgXmlSaxLibrary"/>
		<rdfs:subClassOf rdf:resource="&j2se-1_5;JavaxPrintLibrary"/>
		<rdfs:subClassOf rdf:resource="&j2se-1_5;JavaAwtDatatransferLibrary"/>
		<rdfs:subClassOf rdf:resource="&j2se-1_5;JavaSecurityCertLibrary"/>
		<rdfs:subClassOf rdf:resource="&j2se-1_5;JavaxXmlValidationLibrary"/>
		<rdfs:subClassOf rdf:resource="&j2se-1_5;JavaAwtDndLibrary"/>
		<rdfs:subClassOf rdf:resource="&j2se-1_5;JavaxXmlTransformSaxLibrary"/>
		<rdfs:subClassOf rdf:resource="&j2se-1_5;JavaUtilPrefsLibrary"/>
		<rdfs:subClassOf rdf:resource="&j2se-1_5;JavaMathLibrary"/>
		<rdfs:subClassOf rdf:resource="&j2se-1_5;JavaAwtDndPeerLibrary"/>
		<rdfs:subClassOf rdf:resource="&j2se-1_5;JavaxNamingSpiLibrary"/>
		<rdfs:subClassOf rdf:resource="&j2se-1_5;OrgW3cDomTraversalLibrary"/>
		<rdfs:subClassOf rdf:resource="&j2se-1_5;JavaxImageioLibrary"/>
		<rdfs:subClassOf rdf:resource="&j2se-1_5;JavaxRmiCORBALibrary"/>
		<rdfs:subClassOf rdf:resource="&j2se-1_5;JavaxXmlNamespaceLibrary"/>
		<rdfs:subClassOf rdf:resource="&j2se-1_5;JavaSqlLibrary"/>
		<rdfs:subClassOf rdf:resource="&j2se-1_5;JavaxManagementLoadingLibrary"/>
		<rdfs:subClassOf rdf:resource="&j2se-1_5;OrgOmgStubJavaxManagementRemoteRmiLibrary"/>
		<rdfs:subClassOf rdf:resource="&j2se-1_5;JavaxPrintAttributeLibrary"/>
		<rdfs:subClassOf rdf:resource="&j2se-1_5;JavaxActivityLibrary"/>
		<rdfs:subClassOf rdf:resource="&j2se-1_5;JavaxPrintEventLibrary"/>
		<rdfs:subClassOf rdf:resource="&j2se-1_5;JavaxManagementRemoteRmiLibrary"/>
		<rdfs:subClassOf rdf:resource="&j2se-1_5;JavaxImageioPluginsJpegLibrary"/>
		<rdfs:subClassOf rdf:resource="&j2se-1_5;JavaUtilLibrary"/>
		<rdfs:subClassOf rdf:resource="&j2se-1_5;OrgOmgDynamicAnyLibrary"/>
		<rdfs:subClassOf rdf:resource="&j2se-1_5;JavaxSwingFilechooserLibrary"/>
		<rdfs:subClassOf rdf:resource="&j2se-1_5;JavaNioChannelsSpiLibrary"/>
		<rdfs:subClassOf rdf:resource="&j2se-1_5;OrgOmgCosNamingLibrary"/>
		<rdfs:subClassOf rdf:resource="&j2se-1_5;OrgXmlSaxExtLibrary"/>
		<rdfs:subClassOf rdf:resource="&j2se-1_5;JavaxTransactionLibrary"/>
		<rdfs:subClassOf rdf:resource="&j2se-1_5;JavaxPrintAttributeStandardLibrary"/>
		<rdfs:subClassOf rdf:resource="&j2se-1_5;JavaxAccessibilityLibrary"/>
		<rdfs:subClassOf rdf:resource="&j2se-1_5;JavaxImageioSpiLibrary"/>
		<rdfs:subClassOf rdf:resource="&j2se-1_5;JavaBeansLibrary"/>
		<rdfs:subClassOf rdf:resource="&j2se-1_5;JavaxImageioMetadataLibrary"/>
		<rdfs:subClassOf rdf:resource="&j2se-1_5;JavaRmiRegistryLibrary"/>
		<rdfs:subClassOf rdf:resource="&j2se-1_5;JavaLangLibrary"/>
		<rdfs:subClassOf rdf:resource="&j2se-1_5;JavaxSwingEventLibrary"/>
		<rdfs:subClassOf rdf:resource="&j2se-1_5;JavaxSecurityAuthCallbackLibrary"/>
		<rdfs:subClassOf rdf:resource="&j2se-1_5;OrgW3cDomBootstrapLibrary"/>
		<rdfs:subClassOf rdf:resource="&j2se-1_5;OrgOmgCosNamingNamingContextPackageLibrary"/>
		<rdfs:subClassOf rdf:resource="&j2se-1_5;JavaTextLibrary"/>
		<rdfs:subClassOf rdf:resource="&j2se-1_5;OrgW3cDomLibrary"/>
		<rdfs:subClassOf rdf:resource="&j2se-1_5;JavaxXmlLibrary"/>
		<rdfs:subClassOf rdf:resource="&j2se-1_5;JavaNioCharsetLibrary"/>
		<rdfs:subClassOf rdf:resource="&j2se-1_5;OrgOmgDynamicAnyDynAnyFactoryPackageLibrary"/>
		<rdfs:subClassOf rdf:resource="&j2se-1_5;OrgOmgSendingContextLibrary"/>
		<rdfs:subClassOf rdf:resource="&j2se-1_5;OrgOmgPortableInterceptorLibrary"/>
		<rdfs:subClassOf rdf:resource="&j2se-1_5;JavaxNamingLdapLibrary"/>
		<rdfs:subClassOf rdf:resource="&j2se-1_5;JavaLangReflectLibrary"/>
		<rdfs:subClassOf rdf:resource="&j2se-1_5;JavaxSwingTextHtmlLibrary"/>
		<rdfs:subClassOf rdf:resource="&j2se-1_5;JavaxXmlXpathLibrary"/>
		<rdfs:subClassOf rdf:resource="&j2se-1_5;JavaxSoundMidiSpiLibrary"/>
		<rdfs:subClassOf rdf:resource="&j2se-1_5;JavaxSecurityAuthLoginLibrary"/>
		<rdfs:subClassOf rdf:resource="&j2se-1_5;OrgOmgPortableServerPortableLibrary"/>
		<rdfs:subClassOf rdf:resource="&j2se-1_5;OrgOmgCORBA_2_3Library"/>
		<rdfs:subClassOf rdf:resource="&j2se-1_5;JavaxSwingTableLibrary"/>
		<rdfs:subClassOf rdf:resource="&j2se-1_5;JavaxNamingDirectoryLibrary"/>
		<rdfs:subClassOf rdf:resource="&j2se-1_5;JavaxSwingPlafLibrary"/>
		<rdfs:subClassOf rdf:resource="&j2se-1_5;OrgOmgStubJavaRmiLibrary"/>
		<rdfs:subClassOf rdf:resource="&j2se-1_5;JavaxCryptoLibrary"/>
		<rdfs:subClassOf rdf:resource="&j2se-1_5;OrgW3cDomViewsLibrary"/>
		<rdfs:subClassOf rdf:resource="&j2se-1_5;JavaxSwingPlafSynthLibrary"/>
		<rdfs:subClassOf rdf:resource="&j2se-1_5;JavaLangManagementLibrary"/>
		<rdfs:subClassOf rdf:resource="&j2se-1_5;JavaxSwingBorderLibrary"/>
		<rdfs:subClassOf rdf:resource="&j2se-1_5;OrgW3cDomRangesLibrary"/>
		<rdfs:subClassOf rdf:resource="&j2se-1_5;JavaxSecurityAuthKerberosLibrary"/>
		<rdfs:subClassOf rdf:resource="&j2se-1_5;JavaxSwingLibrary"/>
		<rdfs:subClassOf rdf:resource="&j2se-1_5;JavaLangInstrumentLibrary"/>
		<rdfs:subClassOf rdf:resource="&j2se-1_5;JavaxTransactionXaLibrary"/>
		<rdfs:subClassOf rdf:resource="&j2se-1_5;JavaAppletLibrary"/>
		<rdfs:subClassOf rdf:resource="&j2se-1_5;JavaxSwingTextLibrary"/>
		<rdfs:subClassOf rdf:resource="&j2se-1_5;JavaNioLibrary"/>
		<rdfs:subClassOf rdf:resource="&j2se-1_5;JavaxSoundMidiLibrary"/>
		<rdfs:subClassOf rdf:resource="&j2se-1_5;JavaUtilLoggingLibrary"/>
		<rdfs:subClassOf rdf:resource="&j2se-1_5;OrgW3cDomEventsLibrary"/>
		<rdfs:subClassOf rdf:resource="&j2se-1_5;JavaxSqlRowsetLibrary"/>
		<rdfs:subClassOf rdf:resource="&j2se-1_5;JavaRmiDgcLibrary"/>
		<rdfs:subClassOf rdf:resource="&j2se-1_5;JavaxSqlRowsetSpiLibrary"/>
		<rdfs:subClassOf rdf:resource="&j2se-1_5;JavaSecurityInterfacesLibrary"/>
		<rdfs:subClassOf rdf:resource="&j2se-1_5;JavaxManagementMonitorLibrary"/>
		<rdfs:subClassOf rdf:resource="&j2se-1_5;OrgOmgPortableServerServantLocatorPackageLibrary"/>
		<rdfs:subClassOf rdf:resource="&j2se-1_5;JavaxXmlParsersLibrary"/>
		<rdfs:subClassOf rdf:resource="&j2se-1_5;JavaNetLibrary"/>
		<rdfs:subClassOf rdf:resource="&j2se-1_5;OrgOmgPortableServerLibrary"/>
		<rdfs:subClassOf rdf:resource="&j2se-1_5;OrgW3cDomCssLibrary"/>
		<rdfs:subClassOf rdf:resource="&j2se-1_5;JavaxSwingUndoLibrary"/>
		<rdfs:subClassOf rdf:resource="&j2se-1_5;JavaxSoundSampledSpiLibrary"/>
		<rdfs:subClassOf rdf:resource="&j2se-1_5;JavaxSecurityAuthSpiLibrary"/>
		<rdfs:subClassOf rdf:resource="&j2se-1_5;OrgOmgDynamicAnyDynAnyPackageLibrary"/>
		<rdfs:subClassOf rdf:resource="&j2se-1_5;OrgOmgPortableServerCurrentPackageLibrary"/>
		<rdfs:subClassOf rdf:resource="&j2se-1_5;OrgOmgCosNamingNamingContextExtPackageLibrary"/>
		<rdfs:subClassOf rdf:resource="&j2se-1_5;JavaAwtColorLibrary"/>
		<rdfs:subClassOf rdf:resource="&j2se-1_5;OrgOmgCORBAORBPackageLibrary"/>
		<rdfs:subClassOf rdf:resource="&j2se-1_5;JavaxSwingTreeLibrary"/>
		<rdfs:subClassOf rdf:resource="&j2se-1_5;JavaxSoundSampledLibrary"/>
		<rdfs:subClassOf rdf:resource="&j2se-1_5;JavaUtilConcurrentLibrary"/>
		<rdfs:comment xml:lang="en">JavaLibrary implementing the entire API for j2se-1_5</rdfs:comment>
	</owl:Class>
	<owl:Class rdf:about="&j2se-1_5;J2se-1_5">
		<rdfs:subClassOf rdf:resource="&java;JRE"/>
		<rdfs:subClassOf>
			<owl:Restriction>
				<owl:onProperty rdf:resource="&java;providesBuiltinJavaLibrary"/>
				<owl:someValuesFrom rdf:resource="&j2se-1_5;J2se-1_5ClassLibrary"/>
			</owl:Restriction>
		</rdfs:subClassOf>
		<rdfs:comment xml:lang="en">j2se-1_5 Java Runtime Environment</rdfs:comment>
	</owl:Class>
	<owl:Class rdf:about="&j2se-1_5;OrgOmgCORBAPortableLibrary">
		<rdfs:subClassOf rdf:resource="&j2se-1_4;OrgOmgCORBAPortableLibrary"/>
		<rdfs:seeAlso rdf:resource="&j2se-1_5;OrgOmgCORBA_2_3PortableLibrary"/>
		<rdfs:seeAlso rdf:resource="&j2se-1_5;OrgOmgCORBALibrary"/>
		<rdfs:seeAlso rdf:resource="&j2se-1_5;JavaIoLibrary"/>
		<rdfs:seeAlso rdf:resource="&j2se-1_5;JavaLangLibrary"/>
		<rdfs:seeAlso rdf:resource="&j2se-1_5;JavaMathLibrary"/>
		<rdfs:comment xml:lang="en">JavaLibrary implementing the org.omg.CORBA.portable package for j2se-1_5</rdfs:comment>
	</owl:Class>
	<owl:Class rdf:about="&j2se-1_5;JavaxSqlLibrary">
		<owl:equivalentClass rdf:resource="&j2se-1_4;JavaxSqlLibrary"/>
		<rdfs:subClassOf rdf:resource="&java;JavaLibrary"/>
		<rdfs:seeAlso rdf:resource="&j2se-1_5;JavaxTransactionXaLibrary"/>
		<rdfs:seeAlso rdf:resource="&j2se-1_5;JavaIoLibrary"/>
		<rdfs:seeAlso rdf:resource="&j2se-1_5;JavaSqlLibrary"/>
		<rdfs:seeAlso rdf:resource="&j2se-1_5;JavaLangLibrary"/>
		<rdfs:seeAlso rdf:resource="&j2se-1_5;JavaMathLibrary"/>
		<rdfs:seeAlso rdf:resource="&j2se-1_5;JavaUtilLibrary"/>
		<rdfs:comment xml:lang="en">JavaLibrary implementing the javax.sql package for j2se-1_5</rdfs:comment>
	</owl:Class>
	<owl:Class rdf:about="&j2se-1_5;JavaAwtImageLibrary">
		<rdfs:subClassOf rdf:resource="&j2se-1_4;JavaAwtImageLibrary"/>
		<rdfs:seeAlso rdf:resource="&j2se-1_5;JavaAwtGeomLibrary"/>
		<rdfs:seeAlso rdf:resource="&j2se-1_5;JavaLangLibrary"/>
		<rdfs:seeAlso rdf:resource="&j2se-1_5;JavaAwtLibrary"/>
		<rdfs:seeAlso rdf:resource="&j2se-1_5;JavaMathLibrary"/>
		<rdfs:seeAlso rdf:resource="&j2se-1_5;JavaAwtColorLibrary"/>
		<rdfs:seeAlso rdf:resource="&j2se-1_5;JavaUtilLibrary"/>
		<rdfs:comment xml:lang="en">JavaLibrary implementing the java.awt.image package for j2se-1_5</rdfs:comment>
	</owl:Class>
	<owl:Class rdf:about="&j2se-1_5;OrgIetfJgssLibrary">
		<owl:equivalentClass rdf:resource="&j2se-1_4;OrgIetfJgssLibrary"/>
		<rdfs:subClassOf rdf:resource="&java;JavaLibrary"/>
		<rdfs:seeAlso rdf:resource="&j2se-1_5;JavaSecurityLibrary"/>
		<rdfs:seeAlso rdf:resource="&j2se-1_5;JavaNetLibrary"/>
		<rdfs:seeAlso rdf:resource="&j2se-1_5;JavaIoLibrary"/>
		<rdfs:seeAlso rdf:resource="&j2se-1_5;JavaLangLibrary"/>
		<rdfs:comment xml:lang="en">JavaLibrary implementing the org.ietf.jgss package for j2se-1_5</rdfs:comment>
	</owl:Class>
	<owl:Class rdf:about="&j2se-1_5;OrgOmgCORBADynAnyPackageLibrary">
		<owl:equivalentClass rdf:resource="&j2se-1_4;OrgOmgCORBADynAnyPackageLibrary"/>
		<rdfs:subClassOf rdf:resource="&java;JavaLibrary"/>
		<rdfs:seeAlso rdf:resource="&j2se-1_5;OrgOmgCORBALibrary"/>
		<rdfs:seeAlso rdf:resource="&j2se-1_5;JavaLangLibrary"/>
		<rdfs:comment xml:lang="en">JavaLibrary implementing the org.omg.CORBA.DynAnyPackage package for j2se-1_5</rdfs:comment>
	</owl:Class>
	<owl:Class rdf:about="&j2se-1_5;JavaAwtImLibrary">
		<owl:equivalentClass rdf:resource="&j2se-1_4;JavaAwtImLibrary"/>
		<rdfs:subClassOf rdf:resource="&java;JavaLibrary"/>
		<rdfs:seeAlso rdf:resource="&j2se-1_5;JavaAwtLibrary"/>
		<rdfs:seeAlso rdf:resource="&j2se-1_5;JavaLangLibrary"/>
		<rdfs:seeAlso rdf:resource="&j2se-1_5;JavaTextLibrary"/>
		<rdfs:seeAlso rdf:resource="&j2se-1_5;JavaUtilLibrary"/>
		<rdfs:seeAlso rdf:resource="&j2se-1_5;JavaAwtFontLibrary"/>
		<rdfs:comment xml:lang="en">JavaLibrary implementing the java.awt.im package for j2se-1_5</rdfs:comment>
	</owl:Class>
	<owl:Class rdf:about="&j2se-1_5;JavaLangAnnotationLibrary">
		<rdfs:subClassOf rdf:resource="&java;JavaLibrary"/>
		<rdfs:seeAlso rdf:resource="&j2se-1_5;JavaLangReflectLibrary"/>
		<rdfs:seeAlso rdf:resource="&j2se-1_5;JavaLangLibrary"/>
		<rdfs:comment xml:lang="en">JavaLibrary implementing the java.lang.annotation package for j2se-1_5</rdfs:comment>
	</owl:Class>
	<owl:Class rdf:about="&j2se-1_5;OrgOmgIOPCodecFactoryPackageLibrary">
		<owl:equivalentClass rdf:resource="&j2se-1_4;OrgOmgIOPCodecFactoryPackageLibrary"/>
		<rdfs:subClassOf rdf:resource="&java;JavaLibrary"/>
		<rdfs:seeAlso rdf:resource="&j2se-1_5;OrgOmgCORBAPortableLibrary"/>
		<rdfs:seeAlso rdf:resource="&j2se-1_5;OrgOmgCORBALibrary"/>
		<rdfs:seeAlso rdf:resource="&j2se-1_5;JavaLangLibrary"/>
		<rdfs:comment xml:lang="en">JavaLibrary implementing the org.omg.IOP.CodecFactoryPackage package for j2se-1_5</rdfs:comment>
	</owl:Class>
	<owl:Class rdf:about="&j2se-1_5;JavaxManagementOpenmbeanLibrary">
		<rdfs:subClassOf rdf:resource="&java;JavaLibrary"/>
		<rdfs:seeAlso rdf:resource="&j2se-1_5;JavaIoLibrary"/>
		<rdfs:seeAlso rdf:resource="&j2se-1_5;JavaLangLibrary"/>
		<rdfs:seeAlso rdf:resource="&j2se-1_5;JavaxManagementLibrary"/>
		<rdfs:seeAlso rdf:resource="&j2se-1_5;JavaUtilLibrary"/>
		<rdfs:comment xml:lang="en">JavaLibrary implementing the javax.management.openmbean package for j2se-1_5</rdfs:comment>
	</owl:Class>
	<owl:Class rdf:about="&j2se-1_5;JavaBeansBeancontextLibrary">
		<owl:equivalentClass rdf:resource="&j2se-1_4;JavaBeansBeancontextLibrary"/>
		<rdfs:subClassOf rdf:resource="&java;JavaLibrary"/>
		<rdfs:seeAlso rdf:resource="&j2se-1_5;JavaUtilLibrary"/>
		<rdfs:seeAlso rdf:resource="&j2se-1_5;JavaBeansLibrary"/>
		<rdfs:seeAlso rdf:resource="&j2se-1_5;JavaIoLibrary"/>
		<rdfs:seeAlso rdf:resource="&j2se-1_5;JavaLangLibrary"/>
		<rdfs:seeAlso rdf:resource="&j2se-1_5;JavaAwtLibrary"/>
		<rdfs:seeAlso rdf:resource="&j2se-1_5;JavaNetLibrary"/>
		<rdfs:comment xml:lang="en">JavaLibrary implementing the java.beans.beancontext package for j2se-1_5</rdfs:comment>
	</owl:Class>
	<owl:Class rdf:about="&j2se-1_5;JavaUtilZipLibrary">
		<rdfs:subClassOf rdf:resource="&j2se-1_4;JavaUtilZipLibrary"/>
		<rdfs:seeAlso rdf:resource="&j2se-1_5;JavaIoLibrary"/>
		<rdfs:seeAlso rdf:resource="&j2se-1_5;JavaLangLibrary"/>
		<rdfs:seeAlso rdf:resource="&j2se-1_5;JavaUtilLibrary"/>
		<rdfs:comment xml:lang="en">JavaLibrary implementing the java.util.zip package for j2se-1_5</rdfs:comment>
	</owl:Class>
	<owl:Class rdf:about="&j2se-1_5;JavaxSwingTextHtmlParserLibrary">
		<owl:equivalentClass rdf:resource="&j2se-1_4;JavaxSwingTextHtmlParserLibrary"/>
		<rdfs:subClassOf rdf:resource="&java;JavaLibrary"/>
		<rdfs:seeAlso rdf:resource="&j2se-1_5;JavaxSwingTextHtmlLibrary"/>
		<rdfs:seeAlso rdf:resource="&j2se-1_5;JavaIoLibrary"/>
		<rdfs:seeAlso rdf:resource="&j2se-1_5;JavaxSwingTextLibrary"/>
		<rdfs:seeAlso rdf:resource="&j2se-1_5;JavaLangLibrary"/>
		<rdfs:seeAlso rdf:resource="&j2se-1_5;JavaUtilLibrary"/>
		<rdfs:comment xml:lang="en">JavaLibrary implementing the javax.swing.text.html.parser package for j2se-1_5</rdfs:comment>
	</owl:Class>
	<owl:Class rdf:about="&j2se-1_5;JavaAwtImSpiLibrary">
		<owl:equivalentClass rdf:resource="&j2se-1_4;JavaAwtImSpiLibrary"/>
		<rdfs:subClassOf rdf:resource="&java;JavaLibrary"/>
		<rdfs:seeAlso rdf:resource="&j2se-1_5;JavaAwtImLibrary"/>
		<rdfs:seeAlso rdf:resource="&j2se-1_5;JavaAwtLibrary"/>
		<rdfs:seeAlso rdf:resource="&j2se-1_5;JavaxSwingLibrary"/>
		<rdfs:seeAlso rdf:resource="&j2se-1_5;JavaLangLibrary"/>
		<rdfs:seeAlso rdf:resource="&j2se-1_5;JavaUtilLibrary"/>
		<rdfs:seeAlso rdf:resource="&j2se-1_5;JavaTextLibrary"/>
		<rdfs:seeAlso rdf:resource="&j2se-1_5;JavaAwtFontLibrary"/>
		<rdfs:comment xml:lang="en">JavaLibrary implementing the java.awt.im.spi package for j2se-1_5</rdfs:comment>
	</owl:Class>
	<owl:Class rdf:about="&j2se-1_5;JavaxXmlTransformDomLibrary">
		<rdfs:subClassOf rdf:resource="&j2se-1_4;JavaxXmlTransformDomLibrary"/>
		<rdfs:seeAlso rdf:resource="&j2se-1_5;JavaxXmlTransformLibrary"/>
		<rdfs:seeAlso rdf:resource="&j2se-1_5;JavaLangLibrary"/>
		<rdfs:seeAlso rdf:resource="&j2se-1_5;OrgW3cDomLibrary"/>
		<rdfs:comment xml:lang="en">JavaLibrary implementing the javax.xml.transform.dom package for j2se-1_5</rdfs:comment>
	</owl:Class>
	<owl:Class rdf:about="&j2se-1_5;JavaSecuritySpecLibrary">
		<rdfs:subClassOf rdf:resource="&j2se-1_4;JavaSecuritySpecLibrary"/>
		<rdfs:seeAlso rdf:resource="&j2se-1_5;JavaSecurityInterfacesLibrary"/>
		<rdfs:seeAlso rdf:resource="&j2se-1_5;JavaSecurityLibrary"/>
		<rdfs:seeAlso rdf:resource="&j2se-1_5;JavaMathLibrary"/>
		<rdfs:seeAlso rdf:resource="&j2se-1_5;JavaLangLibrary"/>
		<rdfs:comment xml:lang="en">JavaLibrary implementing the java.security.spec package for j2se-1_5</rdfs:comment>
	</owl:Class>
	<owl:Class rdf:about="&j2se-1_5;JavaUtilJarLibrary">
		<rdfs:subClassOf rdf:resource="&j2se-1_4;JavaUtilJarLibrary"/>
		<rdfs:seeAlso rdf:resource="&j2se-1_5;JavaBeansLibrary"/>
		<rdfs:seeAlso rdf:resource="&j2se-1_5;JavaIoLibrary"/>
		<rdfs:seeAlso rdf:resource="&j2se-1_5;JavaLangLibrary"/>
		<rdfs:seeAlso rdf:resource="&j2se-1_5;JavaUtilZipLibrary"/>
		<rdfs:seeAlso rdf:resource="&j2se-1_5;JavaUtilLibrary"/>
		<rdfs:comment xml:lang="en">JavaLibrary implementing the java.util.jar package for j2se-1_5</rdfs:comment>
	</owl:Class>
	<owl:Class rdf:about="&j2se-1_5;JavaSecurityLibrary">
		<rdfs:subClassOf rdf:resource="&j2se-1_4;JavaSecurityLibrary"/>
		<rdfs:seeAlso rdf:resource="&j2se-1_5;JavaSecuritySpecLibrary"/>
		<rdfs:seeAlso rdf:resource="&j2se-1_5;JavaxCryptoLibrary"/>
		<rdfs:seeAlso rdf:resource="&j2se-1_5;JavaUtilLibrary"/>
		<rdfs:seeAlso rdf:resource="&j2se-1_5;JavaxSecurityAuthLibrary"/>
		<rdfs:seeAlso rdf:resource="&j2se-1_5;JavaIoLibrary"/>
		<rdfs:seeAlso rdf:resource="&j2se-1_5;JavaNioLibrary"/>
		<rdfs:seeAlso rdf:resource="&j2se-1_5;JavaLangLibrary"/>
		<rdfs:seeAlso rdf:resource="&j2se-1_5;JavaxSecurityAuthCallbackLibrary"/>
		<rdfs:seeAlso rdf:resource="&j2se-1_5;JavaSecurityCertLibrary"/>
		<rdfs:seeAlso rdf:resource="&j2se-1_5;JavaNetLibrary"/>
		<rdfs:comment xml:lang="en">JavaLibrary implementing the java.security package for j2se-1_5</rdfs:comment>
	</owl:Class>
	<owl:Class rdf:about="&j2se-1_5;JavaxImageioEventLibrary">
		<owl:equivalentClass rdf:resource="&j2se-1_4;JavaxImageioEventLibrary"/>
		<rdfs:subClassOf rdf:resource="&java;JavaLibrary"/>
		<rdfs:seeAlso rdf:resource="&j2se-1_5;JavaAwtImageLibrary"/>
		<rdfs:seeAlso rdf:resource="&j2se-1_5;JavaxImageioLibrary"/>
		<rdfs:seeAlso rdf:resource="&j2se-1_5;JavaLangLibrary"/>
		<rdfs:seeAlso rdf:resource="&j2se-1_5;JavaUtilLibrary"/>
		<rdfs:comment xml:lang="en">JavaLibrary implementing the javax.imageio.event package for j2se-1_5</rdfs:comment>
	</owl:Class>
	<owl:Class rdf:about="&j2se-1_5;JavaxSwingPlafMultiLibrary">
		<rdfs:subClassOf rdf:resource="&j2se-1_4;JavaxSwingPlafMultiLibrary"/>
		<rdfs:seeAlso rdf:resource="&j2se-1_5;JavaUtilLibrary"/>
		<rdfs:seeAlso rdf:resource="&j2se-1_5;JavaxSwingFilechooserLibrary"/>
		<rdfs:seeAlso rdf:resource="&j2se-1_5;JavaxAccessibilityLibrary"/>
		<rdfs:seeAlso rdf:resource="&j2se-1_5;JavaLangLibrary"/>
		<rdfs:seeAlso rdf:resource="&j2se-1_5;JavaAwtLibrary"/>
		<rdfs:seeAlso rdf:resource="&j2se-1_5;JavaxSwingPlafLibrary"/>
		<rdfs:seeAlso rdf:resource="&j2se-1_5;JavaxSwingLibrary"/>
		<rdfs:seeAlso rdf:resource="&j2se-1_5;JavaIoLibrary"/>
		<rdfs:seeAlso rdf:resource="&j2se-1_5;JavaAwtEventLibrary"/>
		<rdfs:seeAlso rdf:resource="&j2se-1_5;JavaxSwingTextLibrary"/>
		<rdfs:seeAlso rdf:resource="&j2se-1_5;JavaxSwingTreeLibrary"/>
		<rdfs:comment xml:lang="en">JavaLibrary implementing the javax.swing.plaf.multi package for j2se-1_5</rdfs:comment>
	</owl:Class>
	<owl:Class rdf:about="&j2se-1_5;JavaAwtPrintLibrary">
		<owl:equivalentClass rdf:resource="&j2se-1_4;JavaAwtPrintLibrary"/>
		<rdfs:subClassOf rdf:resource="&java;JavaLibrary"/>
		<rdfs:seeAlso rdf:resource="&j2se-1_5;JavaxPrintLibrary"/>
		<rdfs:seeAlso rdf:resource="&j2se-1_5;JavaAwtLibrary"/>
		<rdfs:seeAlso rdf:resource="&j2se-1_5;JavaIoLibrary"/>
		<rdfs:seeAlso rdf:resource="&j2se-1_5;JavaLangLibrary"/>
		<rdfs:seeAlso rdf:resource="&j2se-1_5;JavaxPrintAttributeLibrary"/>
		<rdfs:comment xml:lang="en">JavaLibrary implementing the java.awt.print package for j2se-1_5</rdfs:comment>
	</owl:Class>
	<owl:Class rdf:about="&j2se-1_5;JavaxXmlTransformStreamLibrary">
		<owl:equivalentClass rdf:resource="&j2se-1_4;JavaxXmlTransformStreamLibrary"/>
		<rdfs:subClassOf rdf:resource="&java;JavaLibrary"/>
		<rdfs:seeAlso rdf:resource="&j2se-1_5;JavaxXmlTransformLibrary"/>
		<rdfs:seeAlso rdf:resource="&j2se-1_5;JavaIoLibrary"/>
		<rdfs:seeAlso rdf:resource="&j2se-1_5;JavaLangLibrary"/>
		<rdfs:comment xml:lang="en">JavaLibrary implementing the javax.xml.transform.stream package for j2se-1_5</rdfs:comment>
	</owl:Class>
	<owl:Class rdf:about="&j2se-1_5;JavaxNamingEventLibrary">
		<owl:equivalentClass rdf:resource="&j2se-1_4;JavaxNamingEventLibrary"/>
		<rdfs:subClassOf rdf:resource="&java;JavaLibrary"/>
		<rdfs:seeAlso rdf:resource="&j2se-1_5;JavaxNamingDirectoryLibrary"/>
		<rdfs:seeAlso rdf:resource="&j2se-1_5;JavaxNamingLibrary"/>
		<rdfs:seeAlso rdf:resource="&j2se-1_5;JavaLangLibrary"/>
		<rdfs:seeAlso rdf:resource="&j2se-1_5;JavaUtilLibrary"/>
		<rdfs:comment xml:lang="en">JavaLibrary implementing the javax.naming.event package for j2se-1_5</rdfs:comment>
	</owl:Class>
	<owl:Class rdf:about="&j2se-1_5;JavaxSecuritySaslLibrary">
		<rdfs:subClassOf rdf:resource="&java;JavaLibrary"/>
		<rdfs:seeAlso rdf:resource="&j2se-1_5;JavaIoLibrary"/>
		<rdfs:seeAlso rdf:resource="&j2se-1_5;JavaLangLibrary"/>
		<rdfs:seeAlso rdf:resource="&j2se-1_5;JavaUtilLibrary"/>
		<rdfs:seeAlso rdf:resource="&j2se-1_5;JavaxSecurityAuthCallbackLibrary"/>
		<rdfs:comment xml:lang="en">JavaLibrary implementing the javax.security.sasl package for j2se-1_5</rdfs:comment>
	</owl:Class>
	<owl:Class rdf:about="&j2se-1_5;OrgOmgIOPCodecPackageLibrary">
		<owl:equivalentClass rdf:resource="&j2se-1_4;OrgOmgIOPCodecPackageLibrary"/>
		<rdfs:subClassOf rdf:resource="&java;JavaLibrary"/>
		<rdfs:seeAlso rdf:resource="&j2se-1_5;OrgOmgCORBAPortableLibrary"/>
		<rdfs:seeAlso rdf:resource="&j2se-1_5;OrgOmgCORBALibrary"/>
		<rdfs:seeAlso rdf:resource="&j2se-1_5;JavaLangLibrary"/>
		<rdfs:comment xml:lang="en">JavaLibrary implementing the org.omg.IOP.CodecPackage package for j2se-1_5</rdfs:comment>
	</owl:Class>
	<owl:Class rdf:about="&j2se-1_5;JavaNioCharsetSpiLibrary">
		<owl:equivalentClass rdf:resource="&j2se-1_4;JavaNioCharsetSpiLibrary"/>
		<rdfs:subClassOf rdf:resource="&java;JavaLibrary"/>
		<rdfs:seeAlso rdf:resource="&j2se-1_5;JavaLangLibrary"/>
		<rdfs:seeAlso rdf:resource="&j2se-1_5;JavaUtilLibrary"/>
		<rdfs:seeAlso rdf:resource="&j2se-1_5;JavaNioCharsetLibrary"/>
		<rdfs:comment xml:lang="en">JavaLibrary implementing the java.nio.charset.spi package for j2se-1_5</rdfs:comment>
	</owl:Class>
	<owl:Class rdf:about="&j2se-1_5;JavaxXmlTransformLibrary">
		<rdfs:subClassOf rdf:resource="&j2se-1_4;JavaxXmlTransformLibrary"/>
		<rdfs:seeAlso rdf:resource="&j2se-1_5;JavaIoLibrary"/>
		<rdfs:seeAlso rdf:resource="&j2se-1_5;JavaLangLibrary"/>
		<rdfs:seeAlso rdf:resource="&j2se-1_5;JavaUtilLibrary"/>
		<rdfs:comment xml:lang="en">JavaLibrary implementing the javax.xml.transform package for j2se-1_5</rdfs:comment>
	</owl:Class>
	<owl:Class rdf:about="&j2se-1_5;OrgOmgPortableInterceptorORBInitInfoPackageLibrary">
		<owl:equivalentClass rdf:resource="&j2se-1_4;OrgOmgPortableInterceptorORBInitInfoPackageLibrary"/>
		<rdfs:subClassOf rdf:resource="&java;JavaLibrary"/>
		<rdfs:seeAlso rdf:resource="&j2se-1_5;OrgOmgCORBAPortableLibrary"/>
		<rdfs:seeAlso rdf:resource="&j2se-1_5;OrgOmgCORBALibrary"/>
		<rdfs:seeAlso rdf:resource="&j2se-1_5;JavaLangLibrary"/>
		<rdfs:comment xml:lang="en">JavaLibrary implementing the org.omg.PortableInterceptor.ORBInitInfoPackage package for j2se-1_5</rdfs:comment>
	</owl:Class>
	<owl:Class rdf:about="&j2se-1_5;JavaLangRefLibrary">
		<owl:equivalentClass rdf:resource="&j2se-1_4;JavaLangRefLibrary"/>
		<rdfs:subClassOf rdf:resource="&java;JavaLibrary"/>
		<rdfs:seeAlso rdf:resource="&j2se-1_5;JavaLangLibrary"/>
		<rdfs:comment xml:lang="en">JavaLibrary implementing the java.lang.ref package for j2se-1_5</rdfs:comment>
	</owl:Class>
	<owl:Class rdf:about="&j2se-1_5;JavaxSecurityAuthLibrary">
		<owl:equivalentClass rdf:resource="&j2se-1_4;JavaxSecurityAuthLibrary"/>
		<rdfs:subClassOf rdf:resource="&java;JavaLibrary"/>
		<rdfs:seeAlso rdf:resource="&j2se-1_5;JavaIoLibrary"/>
		<rdfs:seeAlso rdf:resource="&j2se-1_5;JavaLangLibrary"/>
		<rdfs:seeAlso rdf:resource="&j2se-1_5;JavaSecurityLibrary"/>
		<rdfs:seeAlso rdf:resource="&j2se-1_5;JavaUtilLibrary"/>
		<rdfs:comment xml:lang="en">JavaLibrary implementing the javax.security.auth package for j2se-1_5</rdfs:comment>
	</owl:Class>
	<owl:Class rdf:about="&j2se-1_5;JavaxSqlRowsetSerialLibrary">
		<rdfs:subClassOf rdf:resource="&java;JavaLibrary"/>
		<rdfs:seeAlso rdf:resource="&j2se-1_5;JavaSqlLibrary"/>
		<rdfs:seeAlso rdf:resource="&j2se-1_5;JavaUtilLibrary"/>
		<rdfs:seeAlso rdf:resource="&j2se-1_5;JavaIoLibrary"/>
		<rdfs:seeAlso rdf:resource="&j2se-1_5;JavaLangLibrary"/>
		<rdfs:seeAlso rdf:resource="&j2se-1_5;JavaNetLibrary"/>
		<rdfs:seeAlso rdf:resource="&j2se-1_5;JavaMathLibrary"/>
		<rdfs:comment xml:lang="en">JavaLibrary implementing the javax.sql.rowset.serial package for j2se-1_5</rdfs:comment>
	</owl:Class>
	<owl:Class rdf:about="&j2se-1_5;JavaRmiLibrary">
		<owl:equivalentClass rdf:resource="&j2se-1_4;JavaRmiLibrary"/>
		<rdfs:subClassOf rdf:resource="&java;JavaLibrary"/>
		<rdfs:seeAlso rdf:resource="&j2se-1_5;JavaIoLibrary"/>
		<rdfs:seeAlso rdf:resource="&j2se-1_5;JavaLangLibrary"/>
		<rdfs:comment xml:lang="en">JavaLibrary implementing the java.rmi package for j2se-1_5</rdfs:comment>
	</owl:Class>
	<owl:Class rdf:about="&j2se-1_5;JavaxManagementRemoteLibrary">
		<rdfs:subClassOf rdf:resource="&java;JavaLibrary"/>
		<rdfs:seeAlso rdf:resource="&j2se-1_5;JavaxSecurityAuthLibrary"/>
		<rdfs:seeAlso rdf:resource="&j2se-1_5;JavaIoLibrary"/>
		<rdfs:seeAlso rdf:resource="&j2se-1_5;JavaLangLibrary"/>
		<rdfs:seeAlso rdf:resource="&j2se-1_5;JavaxManagementLibrary"/>
		<rdfs:seeAlso rdf:resource="&j2se-1_5;JavaSecurityLibrary"/>
		<rdfs:seeAlso rdf:resource="&j2se-1_5;JavaUtilLibrary"/>
		<rdfs:comment xml:lang="en">JavaLibrary implementing the javax.management.remote package for j2se-1_5</rdfs:comment>
	</owl:Class>
	<owl:Class rdf:about="&j2se-1_5;JavaxManagementLibrary">
		<rdfs:subClassOf rdf:resource="&java;JavaLibrary"/>
		<rdfs:seeAlso rdf:resource="&j2se-1_5;JavaLangReflectLibrary"/>
		<rdfs:seeAlso rdf:resource="&j2se-1_5;JavaxManagementLoadingLibrary"/>
		<rdfs:seeAlso rdf:resource="&j2se-1_5;JavaSecurityLibrary"/>
		<rdfs:seeAlso rdf:resource="&j2se-1_5;JavaUtilLibrary"/>
		<rdfs:seeAlso rdf:resource="&j2se-1_5;JavaIoLibrary"/>
		<rdfs:seeAlso rdf:resource="&j2se-1_5;JavaLangLibrary"/>
		<rdfs:comment xml:lang="en">JavaLibrary implementing the javax.management package for j2se-1_5</rdfs:comment>
	</owl:Class>
	<owl:Class rdf:about="&j2se-1_5;JavaAwtLibrary">
		<rdfs:subClassOf rdf:resource="&j2se-1_4;JavaAwtLibrary"/>
		<rdfs:seeAlso rdf:resource="&j2se-1_5;JavaAwtImageLibrary"/>
		<rdfs:seeAlso rdf:resource="&j2se-1_5;JavaAwtImLibrary"/>
		<rdfs:seeAlso rdf:resource="&j2se-1_5;JavaSecurityLibrary"/>
		<rdfs:seeAlso rdf:resource="&j2se-1_5;JavaAwtFontLibrary"/>
		<rdfs:seeAlso rdf:resource="&j2se-1_5;JavaAwtGeomLibrary"/>
		<rdfs:seeAlso rdf:resource="&j2se-1_5;JavaAwtImageRenderableLibrary"/>
		<rdfs:seeAlso rdf:resource="&j2se-1_5;JavaIoLibrary"/>
		<rdfs:seeAlso rdf:resource="&j2se-1_5;JavaAwtEventLibrary"/>
		<rdfs:seeAlso rdf:resource="&j2se-1_5;JavaAwtPeerLibrary"/>
		<rdfs:seeAlso rdf:resource="&j2se-1_5;JavaAwtDatatransferLibrary"/>
		<rdfs:seeAlso rdf:resource="&j2se-1_5;JavaAwtDndLibrary"/>
		<rdfs:seeAlso rdf:resource="&j2se-1_5;JavaAwtDndPeerLibrary"/>
		<rdfs:seeAlso rdf:resource="&j2se-1_5;JavaUtilLibrary"/>
		<rdfs:seeAlso rdf:resource="&j2se-1_5;JavaxAccessibilityLibrary"/>
		<rdfs:seeAlso rdf:resource="&j2se-1_5;JavaBeansLibrary"/>
		<rdfs:seeAlso rdf:resource="&j2se-1_5;JavaLangLibrary"/>
		<rdfs:seeAlso rdf:resource="&j2se-1_5;JavaTextLibrary"/>
		<rdfs:seeAlso rdf:resource="&j2se-1_5;JavaxSwingTextLibrary"/>
		<rdfs:seeAlso rdf:resource="&j2se-1_5;JavaNetLibrary"/>
		<rdfs:seeAlso rdf:resource="&j2se-1_5;JavaAwtColorLibrary"/>
		<rdfs:comment xml:lang="en">JavaLibrary implementing the java.awt package for j2se-1_5</rdfs:comment>
	</owl:Class>
	<owl:Class rdf:about="&j2se-1_5;JavaxManagementModelmbeanLibrary">
		<rdfs:subClassOf rdf:resource="&java;JavaLibrary"/>
		<rdfs:seeAlso rdf:resource="&j2se-1_5;JavaLangReflectLibrary"/>
		<rdfs:seeAlso rdf:resource="&j2se-1_5;JavaxManagementLoadingLibrary"/>
		<rdfs:seeAlso rdf:resource="&j2se-1_5;JavaIoLibrary"/>
		<rdfs:seeAlso rdf:resource="&j2se-1_5;JavaLangLibrary"/>
		<rdfs:seeAlso rdf:resource="&j2se-1_5;JavaxManagementLibrary"/>
		<rdfs:comment xml:lang="en">JavaLibrary implementing the javax.management.modelmbean package for j2se-1_5</rdfs:comment>
	</owl:Class>
	<owl:Class rdf:about="&j2se-1_5;JavaxSwingTextRtfLibrary">
		<owl:equivalentClass rdf:resource="&j2se-1_4;JavaxSwingTextRtfLibrary"/>
		<rdfs:subClassOf rdf:resource="&java;JavaLibrary"/>
		<rdfs:seeAlso rdf:resource="&j2se-1_5;JavaIoLibrary"/>
		<rdfs:seeAlso rdf:resource="&j2se-1_5;JavaLangLibrary"/>
		<rdfs:seeAlso rdf:resource="&j2se-1_5;JavaxSwingTextLibrary"/>
		<rdfs:comment xml:lang="en">JavaLibrary implementing the javax.swing.text.rtf package for j2se-1_5</rdfs:comment>
	</owl:Class>
	<owl:Class rdf:about="&j2se-1_5;JavaNioChannelsLibrary">
		<rdfs:subClassOf rdf:resource="&j2se-1_4;JavaNioChannelsLibrary"/>
		<rdfs:seeAlso rdf:resource="&j2se-1_5;JavaIoLibrary"/>
		<rdfs:seeAlso rdf:resource="&j2se-1_5;JavaNioLibrary"/>
		<rdfs:seeAlso rdf:resource="&j2se-1_5;JavaLangLibrary"/>
		<rdfs:seeAlso rdf:resource="&j2se-1_5;JavaNetLibrary"/>
		<rdfs:seeAlso rdf:resource="&j2se-1_5;JavaUtilLibrary"/>
		<rdfs:seeAlso rdf:resource="&j2se-1_5;JavaNioCharsetLibrary"/>
		<rdfs:seeAlso rdf:resource="&j2se-1_5;JavaNioChannelsSpiLibrary"/>
		<rdfs:comment xml:lang="en">JavaLibrary implementing the java.nio.channels package for j2se-1_5</rdfs:comment>
	</owl:Class>
	<owl:Class rdf:about="&j2se-1_5;JavaUtilConcurrentLocksLibrary">
		<rdfs:subClassOf rdf:resource="&java;JavaLibrary"/>
		<rdfs:seeAlso rdf:resource="&j2se-1_5;JavaIoLibrary"/>
		<rdfs:seeAlso rdf:resource="&j2se-1_5;JavaLangLibrary"/>
		<rdfs:seeAlso rdf:resource="&j2se-1_5;JavaUtilLibrary"/>
		<rdfs:seeAlso rdf:resource="&j2se-1_5;JavaUtilConcurrentLibrary"/>
		<rdfs:comment xml:lang="en">JavaLibrary implementing the java.util.concurrent.locks package for j2se-1_5</rdfs:comment>
	</owl:Class>
	<owl:Class rdf:about="&j2se-1_5;JavaRmiServerLibrary">
		<rdfs:subClassOf rdf:resource="&j2se-1_4;JavaRmiServerLibrary"/>
		<rdfs:seeAlso rdf:resource="&j2se-1_5;JavaLangReflectLibrary"/>
		<rdfs:seeAlso rdf:resource="&j2se-1_5;JavaRmiLibrary"/>
		<rdfs:seeAlso rdf:resource="&j2se-1_5;JavaIoLibrary"/>
		<rdfs:seeAlso rdf:resource="&j2se-1_5;JavaLangLibrary"/>
		<rdfs:seeAlso rdf:resource="&j2se-1_5;JavaNetLibrary"/>
		<rdfs:comment xml:lang="en">JavaLibrary implementing the java.rmi.server package for j2se-1_5</rdfs:comment>
	</owl:Class>
	<owl:Class rdf:about="&j2se-1_5;OrgW3cDomHtmlLibrary">
		<rdfs:subClassOf rdf:resource="&j2se-1_4;OrgW3cDomHtmlLibrary"/>
		<rdfs:seeAlso rdf:resource="&j2se-1_5;JavaLangLibrary"/>
		<rdfs:seeAlso rdf:resource="&j2se-1_5;OrgW3cDomLibrary"/>
		<rdfs:comment xml:lang="en">JavaLibrary implementing the org.w3c.dom.html package for j2se-1_5</rdfs:comment>
	</owl:Class>
	<owl:Class rdf:about="&j2se-1_5;JavaxSwingColorchooserLibrary">
		<rdfs:subClassOf rdf:resource="&j2se-1_4;JavaxSwingColorchooserLibrary"/>
		<rdfs:seeAlso rdf:resource="&j2se-1_5;JavaxSwingLibrary"/>
		<rdfs:seeAlso rdf:resource="&j2se-1_5;JavaIoLibrary"/>
		<rdfs:seeAlso rdf:resource="&j2se-1_5;JavaLangLibrary"/>
		<rdfs:seeAlso rdf:resource="&j2se-1_5;JavaxSwingEventLibrary"/>
		<rdfs:seeAlso rdf:resource="&j2se-1_5;JavaAwtLibrary"/>
		<rdfs:comment xml:lang="en">JavaLibrary implementing the javax.swing.colorchooser package for j2se-1_5</rdfs:comment>
	</owl:Class>
	<owl:Class rdf:about="&j2se-1_5;OrgOmgPortableServerPOAManagerPackageLibrary">
		<owl:equivalentClass rdf:resource="&j2se-1_4;OrgOmgPortableServerPOAManagerPackageLibrary"/>
		<rdfs:subClassOf rdf:resource="&java;JavaLibrary"/>
		<rdfs:seeAlso rdf:resource="&j2se-1_5;OrgOmgCORBAPortableLibrary"/>
		<rdfs:seeAlso rdf:resource="&j2se-1_5;OrgOmgCORBALibrary"/>
		<rdfs:seeAlso rdf:resource="&j2se-1_5;JavaLangLibrary"/>
		<rdfs:comment xml:lang="en">JavaLibrary implementing the org.omg.PortableServer.POAManagerPackage package for j2se-1_5</rdfs:comment>
	</owl:Class>
	<owl:Class rdf:about="&j2se-1_5;JavaxImageioStreamLibrary">
		<owl:equivalentClass rdf:resource="&j2se-1_4;JavaxImageioStreamLibrary"/>
		<rdfs:subClassOf rdf:resource="&java;JavaLibrary"/>
		<rdfs:seeAlso rdf:resource="&j2se-1_5;JavaIoLibrary"/>
		<rdfs:seeAlso rdf:resource="&j2se-1_5;JavaLangLibrary"/>
		<rdfs:seeAlso rdf:resource="&j2se-1_5;JavaNioLibrary"/>
		<rdfs:comment xml:lang="en">JavaLibrary implementing the javax.imageio.stream package for j2se-1_5</rdfs:comment>
	</owl:Class>
	<owl:Class rdf:about="&j2se-1_5;JavaxXmlDatatypeLibrary">
		<rdfs:subClassOf rdf:resource="&java;JavaLibrary"/>
		<rdfs:seeAlso rdf:resource="&j2se-1_5;JavaxXmlNamespaceLibrary"/>
		<rdfs:seeAlso rdf:resource="&j2se-1_5;JavaLangLibrary"/>
		<rdfs:seeAlso rdf:resource="&j2se-1_5;JavaMathLibrary"/>
		<rdfs:seeAlso rdf:resource="&j2se-1_5;JavaUtilLibrary"/>
		<rdfs:comment xml:lang="en">JavaLibrary implementing the javax.xml.datatype package for j2se-1_5</rdfs:comment>
	</owl:Class>
	<owl:Class rdf:about="&j2se-1_5;JavaxRmiSslLibrary">
		<rdfs:subClassOf rdf:resource="&java;JavaLibrary"/>
		<rdfs:seeAlso rdf:resource="&j2se-1_5;JavaNetLibrary"/>
		<rdfs:seeAlso rdf:resource="&j2se-1_5;JavaRmiServerLibrary"/>
		<rdfs:seeAlso rdf:resource="&j2se-1_5;JavaIoLibrary"/>
		<rdfs:seeAlso rdf:resource="&j2se-1_5;JavaLangLibrary"/>
		<rdfs:comment xml:lang="en">JavaLibrary implementing the javax.rmi.ssl package for j2se-1_5</rdfs:comment>
	</owl:Class>
	<owl:Class rdf:about="&j2se-1_5;JavaxManagementRelationLibrary">
		<rdfs:subClassOf rdf:resource="&java;JavaLibrary"/>
		<rdfs:seeAlso rdf:resource="&j2se-1_5;JavaIoLibrary"/>
		<rdfs:seeAlso rdf:resource="&j2se-1_5;JavaLangLibrary"/>
		<rdfs:seeAlso rdf:resource="&j2se-1_5;JavaxManagementLibrary"/>
		<rdfs:seeAlso rdf:resource="&j2se-1_5;JavaUtilLibrary"/>
		<rdfs:comment xml:lang="en">JavaLibrary implementing the javax.management.relation package for j2se-1_5</rdfs:comment>
	</owl:Class>
	<owl:Class rdf:about="&j2se-1_5;JavaUtilRegexLibrary">
		<rdfs:subClassOf rdf:resource="&j2se-1_4;JavaUtilRegexLibrary"/>
		<rdfs:seeAlso rdf:resource="&j2se-1_5;JavaIoLibrary"/>
		<rdfs:seeAlso rdf:resource="&j2se-1_5;JavaLangLibrary"/>
		<rdfs:comment xml:lang="en">JavaLibrary implementing the java.util.regex package for j2se-1_5</rdfs:comment>
	</owl:Class>
	<owl:Class rdf:about="&j2se-1_5;OrgOmgMessagingLibrary">
		<owl:equivalentClass rdf:resource="&j2se-1_4;OrgOmgMessagingLibrary"/>
		<rdfs:subClassOf rdf:resource="&java;JavaLibrary"/>
		<rdfs:seeAlso rdf:resource="&j2se-1_5;OrgOmgCORBAPortableLibrary"/>
		<rdfs:seeAlso rdf:resource="&j2se-1_5;OrgOmgCORBALibrary"/>
		<rdfs:seeAlso rdf:resource="&j2se-1_5;JavaLangLibrary"/>
		<rdfs:comment xml:lang="en">JavaLibrary implementing the org.omg.Messaging package for j2se-1_5</rdfs:comment>
	</owl:Class>
	<owl:Class rdf:about="&j2se-1_5;JavaxSwingPlafMetalLibrary">
		<rdfs:subClassOf rdf:resource="&j2se-1_4;JavaxSwingPlafMetalLibrary"/>
		<rdfs:seeAlso rdf:resource="&j2se-1_5;JavaBeansLibrary"/>
		<rdfs:seeAlso rdf:resource="&j2se-1_5;JavaLangLibrary"/>
		<rdfs:seeAlso rdf:resource="&j2se-1_5;JavaxSwingEventLibrary"/>
		<rdfs:seeAlso rdf:resource="&j2se-1_5;JavaAwtLibrary"/>
		<rdfs:seeAlso rdf:resource="&j2se-1_5;JavaxSwingPlafLibrary"/>
		<rdfs:seeAlso rdf:resource="&j2se-1_5;JavaxSwingPlafBasicLibrary"/>
		<rdfs:seeAlso rdf:resource="&j2se-1_5;JavaxSwingBorderLibrary"/>
		<rdfs:seeAlso rdf:resource="&j2se-1_5;JavaxSwingLibrary"/>
		<rdfs:seeAlso rdf:resource="&j2se-1_5;JavaIoLibrary"/>
		<rdfs:seeAlso rdf:resource="&j2se-1_5;JavaAwtEventLibrary"/>
		<rdfs:seeAlso rdf:resource="&j2se-1_5;JavaxSwingTreeLibrary"/>
		<rdfs:comment xml:lang="en">JavaLibrary implementing the javax.swing.plaf.metal package for j2se-1_5</rdfs:comment>
	</owl:Class>
	<owl:Class rdf:about="&j2se-1_5;OrgW3cDomStylesheetsLibrary">
		<owl:equivalentClass rdf:resource="&j2se-1_4;OrgW3cDomStylesheetsLibrary"/>
		<rdfs:subClassOf rdf:resource="&java;JavaLibrary"/>
		<rdfs:seeAlso rdf:resource="&j2se-1_5;JavaLangLibrary"/>
		<rdfs:seeAlso rdf:resource="&j2se-1_5;OrgW3cDomLibrary"/>
		<rdfs:comment xml:lang="en">JavaLibrary implementing the org.w3c.dom.stylesheets package for j2se-1_5</rdfs:comment>
	</owl:Class>
	<owl:Class rdf:about="&j2se-1_5;JavaxImageioPluginsBmpLibrary">
		<rdfs:subClassOf rdf:resource="&java;JavaLibrary"/>
		<rdfs:seeAlso rdf:resource="&j2se-1_5;JavaxImageioLibrary"/>
		<rdfs:seeAlso rdf:resource="&j2se-1_5;JavaUtilLibrary"/>
		<rdfs:comment xml:lang="en">JavaLibrary implementing the javax.imageio.plugins.bmp package for j2se-1_5</rdfs:comment>
	</owl:Class>
	<owl:Class rdf:about="&j2se-1_5;OrgXmlSaxHelpersLibrary">
		<rdfs:subClassOf rdf:resource="&j2se-1_4;OrgXmlSaxHelpersLibrary"/>
		<rdfs:seeAlso rdf:resource="&j2se-1_5;JavaLangLibrary"/>
		<rdfs:seeAlso rdf:resource="&j2se-1_5;OrgXmlSaxLibrary"/>
		<rdfs:seeAlso rdf:resource="&j2se-1_5;JavaUtilLibrary"/>
		<rdfs:comment xml:lang="en">JavaLibrary implementing the org.xml.sax.helpers package for j2se-1_5</rdfs:comment>
	</owl:Class>
	<owl:Class rdf:about="&j2se-1_5;JavaxSecurityAuthX500Library">
		<owl:equivalentClass rdf:resource="&j2se-1_4;JavaxSecurityAuthX500Library"/>
		<rdfs:subClassOf rdf:resource="&java;JavaLibrary"/>
		<rdfs:seeAlso rdf:resource="&j2se-1_5;JavaSecurityCertLibrary"/>
		<rdfs:seeAlso rdf:resource="&j2se-1_5;JavaSecurityLibrary"/>
		<rdfs:seeAlso rdf:resource="&j2se-1_5;JavaxSecurityAuthLibrary"/>
		<rdfs:seeAlso rdf:resource="&j2se-1_5;JavaIoLibrary"/>
		<rdfs:seeAlso rdf:resource="&j2se-1_5;JavaLangLibrary"/>
		<rdfs:comment xml:lang="en">JavaLibrary implementing the javax.security.auth.x500 package for j2se-1_5</rdfs:comment>
	</owl:Class>
	<owl:Class rdf:about="&j2se-1_5;OrgOmgIOPLibrary">
		<rdfs:subClassOf rdf:resource="&j2se-1_4;OrgOmgIOPLibrary"/>
		<rdfs:seeAlso rdf:resource="&j2se-1_5;OrgOmgCORBAPortableLibrary"/>
		<rdfs:seeAlso rdf:resource="&j2se-1_5;OrgOmgCORBALibrary"/>
		<rdfs:seeAlso rdf:resource="&j2se-1_5;JavaLangLibrary"/>
		<rdfs:comment xml:lang="en">JavaLibrary implementing the org.omg.IOP package for j2se-1_5</rdfs:comment>
	</owl:Class>
	<owl:Class rdf:about="&j2se-1_5;OrgOmgCORBA_2_3PortableLibrary">
		<owl:equivalentClass rdf:resource="&j2se-1_4;OrgOmgCORBA_2_3PortableLibrary"/>
		<rdfs:subClassOf rdf:resource="&java;JavaLibrary"/>
		<rdfs:seeAlso rdf:resource="&j2se-1_5;OrgOmgCORBAPortableLibrary"/>
		<rdfs:seeAlso rdf:resource="&j2se-1_5;OrgOmgCORBALibrary"/>
		<rdfs:seeAlso rdf:resource="&j2se-1_5;JavaIoLibrary"/>
		<rdfs:seeAlso rdf:resource="&j2se-1_5;JavaLangLibrary"/>
		<rdfs:comment xml:lang="en">JavaLibrary implementing the org.omg.CORBA_2_3.portable package for j2se-1_5</rdfs:comment>
	</owl:Class>
	<owl:Class rdf:about="&j2se-1_5;JavaxNamingLibrary">
		<rdfs:subClassOf rdf:resource="&j2se-1_4;JavaxNamingLibrary"/>
		<rdfs:seeAlso rdf:resource="&j2se-1_5;JavaIoLibrary"/>
		<rdfs:seeAlso rdf:resource="&j2se-1_5;JavaLangLibrary"/>
		<rdfs:seeAlso rdf:resource="&j2se-1_5;JavaUtilLibrary"/>
		<rdfs:comment xml:lang="en">JavaLibrary implementing the javax.naming package for j2se-1_5</rdfs:comment>
	</owl:Class>
	<owl:Class rdf:about="&j2se-1_5;JavaUtilConcurrentAtomicLibrary">
		<rdfs:subClassOf rdf:resource="&java;JavaLibrary"/>
		<rdfs:seeAlso rdf:resource="&j2se-1_5;JavaIoLibrary"/>
		<rdfs:seeAlso rdf:resource="&j2se-1_5;JavaLangLibrary"/>
		<rdfs:comment xml:lang="en">JavaLibrary implementing the java.util.concurrent.atomic package for j2se-1_5</rdfs:comment>
	</owl:Class>
	<owl:Class rdf:about="&j2se-1_5;OrgOmgCORBATypeCodePackageLibrary">
		<owl:equivalentClass rdf:resource="&j2se-1_4;OrgOmgCORBATypeCodePackageLibrary"/>
		<rdfs:subClassOf rdf:resource="&java;JavaLibrary"/>
		<rdfs:seeAlso rdf:resource="&j2se-1_5;OrgOmgCORBALibrary"/>
		<rdfs:seeAlso rdf:resource="&j2se-1_5;JavaLangLibrary"/>
		<rdfs:comment xml:lang="en">JavaLibrary implementing the org.omg.CORBA.TypeCodePackage package for j2se-1_5</rdfs:comment>
	</owl:Class>
	<owl:Class rdf:about="&j2se-1_5;OrgW3cDomLsLibrary">
		<rdfs:subClassOf rdf:resource="&java;JavaLibrary"/>
		<rdfs:seeAlso rdf:resource="&j2se-1_5;OrgW3cDomTraversalLibrary"/>
		<rdfs:seeAlso rdf:resource="&j2se-1_5;JavaIoLibrary"/>
		<rdfs:seeAlso rdf:resource="&j2se-1_5;JavaLangLibrary"/>
		<rdfs:seeAlso rdf:resource="&j2se-1_5;OrgW3cDomEventsLibrary"/>
		<rdfs:seeAlso rdf:resource="&j2se-1_5;OrgW3cDomLibrary"/>
		<rdfs:comment xml:lang="en">JavaLibrary implementing the org.w3c.dom.ls package for j2se-1_5</rdfs:comment>
	</owl:Class>
	<owl:Class rdf:about="&j2se-1_5;OrgOmgCORBALibrary">
		<rdfs:subClassOf rdf:resource="&j2se-1_4;OrgOmgCORBALibrary"/>
		<rdfs:seeAlso rdf:resource="&j2se-1_5;OrgOmgCORBAPortableLibrary"/>
		<rdfs:seeAlso rdf:resource="&j2se-1_5;JavaAppletLibrary"/>
		<rdfs:seeAlso rdf:resource="&j2se-1_5;JavaIoLibrary"/>
		<rdfs:seeAlso rdf:resource="&j2se-1_5;JavaLangLibrary"/>
		<rdfs:seeAlso rdf:resource="&j2se-1_5;JavaMathLibrary"/>
		<rdfs:seeAlso rdf:resource="&j2se-1_5;JavaUtilLibrary"/>
		<rdfs:comment xml:lang="en">JavaLibrary implementing the org.omg.CORBA package for j2se-1_5</rdfs:comment>
	</owl:Class>
	<owl:Class rdf:about="&j2se-1_5;JavaxSwingPlafBasicLibrary">
		<rdfs:subClassOf rdf:resource="&j2se-1_4;JavaxSwingPlafBasicLibrary"/>
		<rdfs:seeAlso rdf:resource="&j2se-1_5;JavaAwtLibrary"/>
		<rdfs:seeAlso rdf:resource="&j2se-1_5;JavaIoLibrary"/>
		<rdfs:seeAlso rdf:resource="&j2se-1_5;JavaAwtEventLibrary"/>
		<rdfs:seeAlso rdf:resource="&j2se-1_5;JavaUtilLibrary"/>
		<rdfs:seeAlso rdf:resource="&j2se-1_5;JavaxSwingFilechooserLibrary"/>
		<rdfs:seeAlso rdf:resource="&j2se-1_5;JavaxAccessibilityLibrary"/>
		<rdfs:seeAlso rdf:resource="&j2se-1_5;JavaBeansLibrary"/>
		<rdfs:seeAlso rdf:resource="&j2se-1_5;JavaLangLibrary"/>
		<rdfs:seeAlso rdf:resource="&j2se-1_5;JavaxSwingEventLibrary"/>
		<rdfs:seeAlso rdf:resource="&j2se-1_5;JavaxSwingTableLibrary"/>
		<rdfs:seeAlso rdf:resource="&j2se-1_5;JavaxSwingPlafLibrary"/>
		<rdfs:seeAlso rdf:resource="&j2se-1_5;JavaxSwingBorderLibrary"/>
		<rdfs:seeAlso rdf:resource="&j2se-1_5;JavaxSwingLibrary"/>
		<rdfs:seeAlso rdf:resource="&j2se-1_5;JavaxSwingTextLibrary"/>
		<rdfs:seeAlso rdf:resource="&j2se-1_5;JavaxSwingTreeLibrary"/>
		<rdfs:comment xml:lang="en">JavaLibrary implementing the javax.swing.plaf.basic package for j2se-1_5</rdfs:comment>
	</owl:Class>
	<owl:Class rdf:about="&j2se-1_5;JavaxManagementTimerLibrary">
		<rdfs:subClassOf rdf:resource="&java;JavaLibrary"/>
		<rdfs:seeAlso rdf:resource="&j2se-1_5;JavaLangLibrary"/>
		<rdfs:seeAlso rdf:resource="&j2se-1_5;JavaxManagementLibrary"/>
		<rdfs:seeAlso rdf:resource="&j2se-1_5;JavaUtilLibrary"/>
		<rdfs:comment xml:lang="en">JavaLibrary implementing the javax.management.timer package for j2se-1_5</rdfs:comment>
	</owl:Class>
	<owl:Class rdf:about="&j2se-1_5;JavaSecurityAclLibrary">
		<owl:equivalentClass rdf:resource="&j2se-1_4;JavaSecurityAclLibrary"/>
		<rdfs:subClassOf rdf:resource="&java;JavaLibrary"/>
		<rdfs:seeAlso rdf:resource="&j2se-1_5;JavaSecurityLibrary"/>
		<rdfs:seeAlso rdf:resource="&j2se-1_5;JavaLangLibrary"/>
		<rdfs:seeAlso rdf:resource="&j2se-1_5;JavaUtilLibrary"/>
		<rdfs:comment xml:lang="en">JavaLibrary implementing the java.security.acl package for j2se-1_5</rdfs:comment>
	</owl:Class>
	<owl:Class rdf:about="&j2se-1_5;JavaAwtFontLibrary">
		<owl:equivalentClass rdf:resource="&j2se-1_4;JavaAwtFontLibrary"/>
		<rdfs:subClassOf rdf:resource="&java;JavaLibrary"/>
		<rdfs:seeAlso rdf:resource="&j2se-1_5;JavaAwtGeomLibrary"/>
		<rdfs:seeAlso rdf:resource="&j2se-1_5;JavaIoLibrary"/>
		<rdfs:seeAlso rdf:resource="&j2se-1_5;JavaLangLibrary"/>
		<rdfs:seeAlso rdf:resource="&j2se-1_5;JavaAwtLibrary"/>
		<rdfs:seeAlso rdf:resource="&j2se-1_5;JavaTextLibrary"/>
		<rdfs:seeAlso rdf:resource="&j2se-1_5;JavaUtilLibrary"/>
		<rdfs:comment xml:lang="en">JavaLibrary implementing the java.awt.font package for j2se-1_5</rdfs:comment>
	</owl:Class>
	<owl:Class rdf:about="&j2se-1_5;OrgOmgDynamicLibrary">
		<owl:equivalentClass rdf:resource="&j2se-1_4;OrgOmgDynamicLibrary"/>
		<rdfs:subClassOf rdf:resource="&java;JavaLibrary"/>
		<rdfs:seeAlso rdf:resource="&j2se-1_5;OrgOmgCORBAPortableLibrary"/>
		<rdfs:seeAlso rdf:resource="&j2se-1_5;OrgOmgCORBALibrary"/>
		<rdfs:seeAlso rdf:resource="&j2se-1_5;JavaLangLibrary"/>
		<rdfs:comment xml:lang="en">JavaLibrary implementing the org.omg.Dynamic package for j2se-1_5</rdfs:comment>
	</owl:Class>
	<owl:Class rdf:about="&j2se-1_5;JavaRmiActivationLibrary">
		<owl:equivalentClass rdf:resource="&j2se-1_4;JavaRmiActivationLibrary"/>
		<rdfs:subClassOf rdf:resource="&java;JavaLibrary"/>
		<rdfs:seeAlso rdf:resource="&j2se-1_5;JavaIoLibrary"/>
		<rdfs:seeAlso rdf:resource="&j2se-1_5;JavaRmiLibrary"/>
		<rdfs:seeAlso rdf:resource="&j2se-1_5;JavaLangLibrary"/>
		<rdfs:seeAlso rdf:resource="&j2se-1_5;JavaRmiServerLibrary"/>
		<rdfs:seeAlso rdf:resource="&j2se-1_5;JavaUtilLibrary"/>
		<rdfs:comment xml:lang="en">JavaLibrary implementing the java.rmi.activation package for j2se-1_5</rdfs:comment>
	</owl:Class>
	<owl:Class rdf:about="&j2se-1_5;JavaAwtGeomLibrary">
		<owl:equivalentClass rdf:resource="&j2se-1_4;JavaAwtGeomLibrary"/>
		<rdfs:subClassOf rdf:resource="&java;JavaLibrary"/>
		<rdfs:seeAlso rdf:resource="&j2se-1_5;JavaAwtLibrary"/>
		<rdfs:seeAlso rdf:resource="&j2se-1_5;JavaIoLibrary"/>
		<rdfs:seeAlso rdf:resource="&j2se-1_5;JavaLangLibrary"/>
		<rdfs:comment xml:lang="en">JavaLibrary implementing the java.awt.geom package for j2se-1_5</rdfs:comment>
	</owl:Class>
	<owl:Class rdf:about="&j2se-1_5;JavaAwtImageRenderableLibrary">
		<owl:equivalentClass rdf:resource="&j2se-1_4;JavaAwtImageRenderableLibrary"/>
		<rdfs:subClassOf rdf:resource="&java;JavaLibrary"/>
		<rdfs:seeAlso rdf:resource="&j2se-1_5;JavaAwtImageLibrary"/>
		<rdfs:seeAlso rdf:resource="&j2se-1_5;JavaAwtGeomLibrary"/>
		<rdfs:seeAlso rdf:resource="&j2se-1_5;JavaIoLibrary"/>
		<rdfs:seeAlso rdf:resource="&j2se-1_5;JavaLangLibrary"/>
		<rdfs:seeAlso rdf:resource="&j2se-1_5;JavaAwtLibrary"/>
		<rdfs:seeAlso rdf:resource="&j2se-1_5;JavaUtilLibrary"/>
		<rdfs:comment xml:lang="en">JavaLibrary implementing the java.awt.image.renderable package for j2se-1_5</rdfs:comment>
	</owl:Class>
	<owl:Class rdf:about="&j2se-1_5;JavaIoLibrary">
		<rdfs:subClassOf rdf:resource="&j2se-1_4;JavaIoLibrary"/>
		<rdfs:seeAlso rdf:resource="&j2se-1_5;JavaNioLibrary"/>
		<rdfs:seeAlso rdf:resource="&j2se-1_5;JavaLangLibrary"/>
		<rdfs:seeAlso rdf:resource="&j2se-1_5;JavaNetLibrary"/>
		<rdfs:seeAlso rdf:resource="&j2se-1_5;JavaNioChannelsLibrary"/>
		<rdfs:seeAlso rdf:resource="&j2se-1_5;JavaSecurityLibrary"/>
		<rdfs:seeAlso rdf:resource="&j2se-1_5;JavaUtilLibrary"/>
		<rdfs:seeAlso rdf:resource="&j2se-1_5;JavaNioCharsetLibrary"/>
		<rdfs:comment xml:lang="en">JavaLibrary implementing the java.io package for j2se-1_5</rdfs:comment>
	</owl:Class>
	<owl:Class rdf:about="&j2se-1_5;JavaAwtEventLibrary">
		<rdfs:subClassOf rdf:resource="&j2se-1_4;JavaAwtEventLibrary"/>
		<rdfs:seeAlso rdf:resource="&j2se-1_5;JavaLangLibrary"/>
		<rdfs:seeAlso rdf:resource="&j2se-1_5;JavaAwtLibrary"/>
		<rdfs:seeAlso rdf:resource="&j2se-1_5;JavaUtilLibrary"/>
		<rdfs:seeAlso rdf:resource="&j2se-1_5;JavaTextLibrary"/>
		<rdfs:seeAlso rdf:resource="&j2se-1_5;JavaAwtFontLibrary"/>
		<rdfs:comment xml:lang="en">JavaLibrary implementing the java.awt.event package for j2se-1_5</rdfs:comment>
	</owl:Class>
	<owl:Class rdf:about="&j2se-1_5;OrgOmgPortableServerPOAPackageLibrary">
		<owl:equivalentClass rdf:resource="&j2se-1_4;OrgOmgPortableServerPOAPackageLibrary"/>
		<rdfs:subClassOf rdf:resource="&java;JavaLibrary"/>
		<rdfs:seeAlso rdf:resource="&j2se-1_5;OrgOmgCORBAPortableLibrary"/>
		<rdfs:seeAlso rdf:resource="&j2se-1_5;OrgOmgCORBALibrary"/>
		<rdfs:seeAlso rdf:resource="&j2se-1_5;JavaLangLibrary"/>
		<rdfs:comment xml:lang="en">JavaLibrary implementing the org.omg.PortableServer.POAPackage package for j2se-1_5</rdfs:comment>
	</owl:Class>
	<owl:Class rdf:about="&j2se-1_5;JavaxRmiLibrary">
		<owl:equivalentClass rdf:resource="&j2se-1_4;JavaxRmiLibrary"/>
		<rdfs:subClassOf rdf:resource="&java;JavaLibrary"/>
		<rdfs:seeAlso rdf:resource="&j2se-1_5;JavaRmiLibrary"/>
		<rdfs:seeAlso rdf:resource="&j2se-1_5;JavaLangLibrary"/>
		<rdfs:comment xml:lang="en">JavaLibrary implementing the javax.rmi package for j2se-1_5</rdfs:comment>
	</owl:Class>
	<owl:Class rdf:about="&j2se-1_5;JavaAwtPeerLibrary">
		<rdfs:subClassOf rdf:resource="&java;JavaLibrary"/>
		<rdfs:seeAlso rdf:resource="&j2se-1_5;JavaAwtImageLibrary"/>
		<rdfs:seeAlso rdf:resource="&j2se-1_5;JavaAwtImLibrary"/>
		<rdfs:seeAlso rdf:resource="&j2se-1_5;JavaIoLibrary"/>
		<rdfs:seeAlso rdf:resource="&j2se-1_5;JavaLangLibrary"/>
		<rdfs:seeAlso rdf:resource="&j2se-1_5;JavaAwtEventLibrary"/>
		<rdfs:seeAlso rdf:resource="&j2se-1_5;JavaAwtLibrary"/>
		<rdfs:comment xml:lang="en">JavaLibrary implementing the java.awt.peer package for j2se-1_5</rdfs:comment>
	</owl:Class>
	<owl:Class rdf:about="&j2se-1_5;OrgXmlSaxLibrary">
		<owl:equivalentClass rdf:resource="&j2se-1_4;OrgXmlSaxLibrary"/>
		<rdfs:subClassOf rdf:resource="&java;JavaLibrary"/>
		<rdfs:seeAlso rdf:resource="&j2se-1_5;JavaIoLibrary"/>
		<rdfs:seeAlso rdf:resource="&j2se-1_5;JavaLangLibrary"/>
		<rdfs:seeAlso rdf:resource="&j2se-1_5;JavaUtilLibrary"/>
		<rdfs:comment xml:lang="en">JavaLibrary implementing the org.xml.sax package for j2se-1_5</rdfs:comment>
	</owl:Class>
	<owl:Class rdf:about="&j2se-1_5;JavaxPrintLibrary">
		<owl:equivalentClass rdf:resource="&j2se-1_4;JavaxPrintLibrary"/>
		<rdfs:subClassOf rdf:resource="&java;JavaLibrary"/>
		<rdfs:seeAlso rdf:resource="&j2se-1_5;JavaIoLibrary"/>
		<rdfs:seeAlso rdf:resource="&j2se-1_5;JavaLangLibrary"/>
		<rdfs:seeAlso rdf:resource="&j2se-1_5;JavaxPrintAttributeLibrary"/>
		<rdfs:seeAlso rdf:resource="&j2se-1_5;JavaAwtLibrary"/>
		<rdfs:seeAlso rdf:resource="&j2se-1_5;JavaxPrintEventLibrary"/>
		<rdfs:seeAlso rdf:resource="&j2se-1_5;JavaNetLibrary"/>
		<rdfs:comment xml:lang="en">JavaLibrary implementing the javax.print package for j2se-1_5</rdfs:comment>
	</owl:Class>
	<owl:Class rdf:about="&j2se-1_5;JavaAwtDatatransferLibrary">
		<rdfs:subClassOf rdf:resource="&j2se-1_4;JavaAwtDatatransferLibrary"/>
		<rdfs:seeAlso rdf:resource="&j2se-1_5;JavaIoLibrary"/>
		<rdfs:seeAlso rdf:resource="&j2se-1_5;JavaLangLibrary"/>
		<rdfs:seeAlso rdf:resource="&j2se-1_5;JavaUtilLibrary"/>
		<rdfs:comment xml:lang="en">JavaLibrary implementing the java.awt.datatransfer package for j2se-1_5</rdfs:comment>
	</owl:Class>
	<owl:Class rdf:about="&j2se-1_5;JavaSecurityCertLibrary">
		<rdfs:subClassOf rdf:resource="&j2se-1_4;JavaSecurityCertLibrary"/>
		<rdfs:seeAlso rdf:resource="&j2se-1_5;JavaIoLibrary"/>
		<rdfs:seeAlso rdf:resource="&j2se-1_5;JavaLangLibrary"/>
		<rdfs:seeAlso rdf:resource="&j2se-1_5;JavaxSecurityAuthX500Library"/>
		<rdfs:seeAlso rdf:resource="&j2se-1_5;JavaSecurityLibrary"/>
		<rdfs:seeAlso rdf:resource="&j2se-1_5;JavaMathLibrary"/>
		<rdfs:seeAlso rdf:resource="&j2se-1_5;JavaUtilLibrary"/>
		<rdfs:comment xml:lang="en">JavaLibrary implementing the java.security.cert package for j2se-1_5</rdfs:comment>
	</owl:Class>
	<owl:Class rdf:about="&j2se-1_5;JavaxXmlValidationLibrary">
		<rdfs:subClassOf rdf:resource="&java;JavaLibrary"/>
		<rdfs:seeAlso rdf:resource="&j2se-1_5;JavaxXmlTransformLibrary"/>
		<rdfs:seeAlso rdf:resource="&j2se-1_5;JavaNetLibrary"/>
		<rdfs:seeAlso rdf:resource="&j2se-1_5;JavaIoLibrary"/>
		<rdfs:seeAlso rdf:resource="&j2se-1_5;OrgW3cDomLsLibrary"/>
		<rdfs:seeAlso rdf:resource="&j2se-1_5;JavaLangLibrary"/>
		<rdfs:seeAlso rdf:resource="&j2se-1_5;OrgW3cDomLibrary"/>
		<rdfs:seeAlso rdf:resource="&j2se-1_5;OrgXmlSaxLibrary"/>
		<rdfs:comment xml:lang="en">JavaLibrary implementing the javax.xml.validation package for j2se-1_5</rdfs:comment>
	</owl:Class>
	<owl:Class rdf:about="&j2se-1_5;JavaAwtDndLibrary">
		<rdfs:subClassOf rdf:resource="&j2se-1_4;JavaAwtDndLibrary"/>
		<rdfs:seeAlso rdf:resource="&j2se-1_5;JavaUtilLibrary"/>
		<rdfs:seeAlso rdf:resource="&j2se-1_5;JavaIoLibrary"/>
		<rdfs:seeAlso rdf:resource="&j2se-1_5;JavaLangLibrary"/>
		<rdfs:seeAlso rdf:resource="&j2se-1_5;JavaAwtEventLibrary"/>
		<rdfs:seeAlso rdf:resource="&j2se-1_5;JavaAwtPeerLibrary"/>
		<rdfs:seeAlso rdf:resource="&j2se-1_5;JavaAwtDatatransferLibrary"/>
		<rdfs:seeAlso rdf:resource="&j2se-1_5;JavaAwtLibrary"/>
		<rdfs:seeAlso rdf:resource="&j2se-1_5;JavaAwtDndPeerLibrary"/>
		<rdfs:comment xml:lang="en">JavaLibrary implementing the java.awt.dnd package for j2se-1_5</rdfs:comment>
	</owl:Class>
	<owl:Class rdf:about="&j2se-1_5;JavaxXmlTransformSaxLibrary">
		<rdfs:subClassOf rdf:resource="&j2se-1_4;JavaxXmlTransformSaxLibrary"/>
		<rdfs:seeAlso rdf:resource="&j2se-1_5;OrgXmlSaxExtLibrary"/>
		<rdfs:seeAlso rdf:resource="&j2se-1_5;JavaxXmlTransformLibrary"/>
		<rdfs:seeAlso rdf:resource="&j2se-1_5;JavaLangLibrary"/>
		<rdfs:seeAlso rdf:resource="&j2se-1_5;OrgXmlSaxLibrary"/>
		<rdfs:comment xml:lang="en">JavaLibrary implementing the javax.xml.transform.sax package for j2se-1_5</rdfs:comment>
	</owl:Class>
	<owl:Class rdf:about="&j2se-1_5;JavaUtilPrefsLibrary">
		<owl:equivalentClass rdf:resource="&j2se-1_4;JavaUtilPrefsLibrary"/>
		<rdfs:subClassOf rdf:resource="&java;JavaLibrary"/>
		<rdfs:seeAlso rdf:resource="&j2se-1_5;JavaIoLibrary"/>
		<rdfs:seeAlso rdf:resource="&j2se-1_5;JavaLangLibrary"/>
		<rdfs:seeAlso rdf:resource="&j2se-1_5;JavaUtilLibrary"/>
		<rdfs:comment xml:lang="en">JavaLibrary implementing the java.util.prefs package for j2se-1_5</rdfs:comment>
	</owl:Class>
	<owl:Class rdf:about="&j2se-1_5;JavaMathLibrary">
		<rdfs:subClassOf rdf:resource="&j2se-1_4;JavaMathLibrary"/>
		<rdfs:seeAlso rdf:resource="&j2se-1_5;JavaIoLibrary"/>
		<rdfs:seeAlso rdf:resource="&j2se-1_5;JavaLangLibrary"/>
		<rdfs:seeAlso rdf:resource="&j2se-1_5;JavaUtilLibrary"/>
		<rdfs:comment xml:lang="en">JavaLibrary implementing the java.math package for j2se-1_5</rdfs:comment>
	</owl:Class>
	<owl:Class rdf:about="&j2se-1_5;JavaAwtDndPeerLibrary">
		<owl:equivalentClass rdf:resource="&j2se-1_4;JavaAwtDndPeerLibrary"/>
		<rdfs:subClassOf rdf:resource="&java;JavaLibrary"/>
		<rdfs:seeAlso rdf:resource="&j2se-1_5;JavaAwtDatatransferLibrary"/>
		<rdfs:seeAlso rdf:resource="&j2se-1_5;JavaAwtLibrary"/>
		<rdfs:seeAlso rdf:resource="&j2se-1_5;JavaAwtDndLibrary"/>
		<rdfs:comment xml:lang="en">JavaLibrary implementing the java.awt.dnd.peer package for j2se-1_5</rdfs:comment>
	</owl:Class>
	<owl:Class rdf:about="&j2se-1_5;JavaxNamingSpiLibrary">
		<owl:equivalentClass rdf:resource="&j2se-1_4;JavaxNamingSpiLibrary"/>
		<rdfs:subClassOf rdf:resource="&java;JavaLibrary"/>
		<rdfs:seeAlso rdf:resource="&j2se-1_5;JavaxNamingDirectoryLibrary"/>
		<rdfs:seeAlso rdf:resource="&j2se-1_5;JavaxNamingLibrary"/>
		<rdfs:seeAlso rdf:resource="&j2se-1_5;JavaIoLibrary"/>
		<rdfs:seeAlso rdf:resource="&j2se-1_5;JavaLangLibrary"/>
		<rdfs:seeAlso rdf:resource="&j2se-1_5;JavaUtilLibrary"/>
		<rdfs:comment xml:lang="en">JavaLibrary implementing the javax.naming.spi package for j2se-1_5</rdfs:comment>
	</owl:Class>
	<owl:Class rdf:about="&j2se-1_5;OrgW3cDomTraversalLibrary">
		<owl:equivalentClass rdf:resource="&j2se-1_4;OrgW3cDomTraversalLibrary"/>
		<rdfs:subClassOf rdf:resource="&java;JavaLibrary"/>
		<rdfs:seeAlso rdf:resource="&j2se-1_5;OrgW3cDomLibrary"/>
		<rdfs:comment xml:lang="en">JavaLibrary implementing the org.w3c.dom.traversal package for j2se-1_5</rdfs:comment>
	</owl:Class>
	<owl:Class rdf:about="&j2se-1_5;JavaxImageioLibrary">
		<owl:equivalentClass rdf:resource="&j2se-1_4;JavaxImageioLibrary"/>
		<rdfs:subClassOf rdf:resource="&java;JavaLibrary"/>
		<rdfs:seeAlso rdf:resource="&j2se-1_5;JavaAwtImageLibrary"/>
		<rdfs:seeAlso rdf:resource="&j2se-1_5;JavaxImageioEventLibrary"/>
		<rdfs:seeAlso rdf:resource="&j2se-1_5;JavaUtilLibrary"/>
		<rdfs:seeAlso rdf:resource="&j2se-1_5;JavaxImageioSpiLibrary"/>
		<rdfs:seeAlso rdf:resource="&j2se-1_5;JavaxImageioMetadataLibrary"/>
		<rdfs:seeAlso rdf:resource="&j2se-1_5;JavaIoLibrary"/>
		<rdfs:seeAlso rdf:resource="&j2se-1_5;JavaLangLibrary"/>
		<rdfs:seeAlso rdf:resource="&j2se-1_5;JavaAwtLibrary"/>
		<rdfs:seeAlso rdf:resource="&j2se-1_5;JavaNetLibrary"/>
		<rdfs:seeAlso rdf:resource="&j2se-1_5;JavaAwtColorLibrary"/>
		<rdfs:seeAlso rdf:resource="&j2se-1_5;JavaxImageioStreamLibrary"/>
		<rdfs:comment xml:lang="en">JavaLibrary implementing the javax.imageio package for j2se-1_5</rdfs:comment>
	</owl:Class>
	<owl:Class rdf:about="&j2se-1_5;JavaxRmiCORBALibrary">
		<rdfs:subClassOf rdf:resource="&j2se-1_4;JavaxRmiCORBALibrary"/>
		<rdfs:seeAlso rdf:resource="&j2se-1_5;OrgOmgSendingContextLibrary"/>
		<rdfs:seeAlso rdf:resource="&j2se-1_5;OrgOmgCORBAPortableLibrary"/>
		<rdfs:seeAlso rdf:resource="&j2se-1_5;JavaRmiLibrary"/>
		<rdfs:seeAlso rdf:resource="&j2se-1_5;JavaIoLibrary"/>
		<rdfs:seeAlso rdf:resource="&j2se-1_5;JavaLangLibrary"/>
		<rdfs:seeAlso rdf:resource="&j2se-1_5;OrgOmgCORBA_2_3PortableLibrary"/>
		<rdfs:seeAlso rdf:resource="&j2se-1_5;OrgOmgCORBALibrary"/>
		<rdfs:comment xml:lang="en">JavaLibrary implementing the javax.rmi.CORBA package for j2se-1_5</rdfs:comment>
	</owl:Class>
	<owl:Class rdf:about="&j2se-1_5;JavaxXmlNamespaceLibrary">
		<rdfs:subClassOf rdf:resource="&java;JavaLibrary"/>
		<rdfs:seeAlso rdf:resource="&j2se-1_5;JavaIoLibrary"/>
		<rdfs:seeAlso rdf:resource="&j2se-1_5;JavaLangLibrary"/>
		<rdfs:seeAlso rdf:resource="&j2se-1_5;JavaUtilLibrary"/>
		<rdfs:comment xml:lang="en">JavaLibrary implementing the javax.xml.namespace package for j2se-1_5</rdfs:comment>
	</owl:Class>
	<owl:Class rdf:about="&j2se-1_5;JavaSqlLibrary">
		<owl:equivalentClass rdf:resource="&j2se-1_4;JavaSqlLibrary"/>
		<rdfs:subClassOf rdf:resource="&java;JavaLibrary"/>
		<rdfs:seeAlso rdf:resource="&j2se-1_5;JavaIoLibrary"/>
		<rdfs:seeAlso rdf:resource="&j2se-1_5;JavaLangLibrary"/>
		<rdfs:seeAlso rdf:resource="&j2se-1_5;JavaNetLibrary"/>
		<rdfs:seeAlso rdf:resource="&j2se-1_5;JavaSecurityLibrary"/>
		<rdfs:seeAlso rdf:resource="&j2se-1_5;JavaMathLibrary"/>
		<rdfs:seeAlso rdf:resource="&j2se-1_5;JavaUtilLibrary"/>
		<rdfs:comment xml:lang="en">JavaLibrary implementing the java.sql package for j2se-1_5</rdfs:comment>
	</owl:Class>
	<owl:Class rdf:about="&j2se-1_5;JavaxManagementLoadingLibrary">
		<rdfs:subClassOf rdf:resource="&java;JavaLibrary"/>
		<rdfs:seeAlso rdf:resource="&j2se-1_5;JavaIoLibrary"/>
		<rdfs:seeAlso rdf:resource="&j2se-1_5;JavaLangLibrary"/>
		<rdfs:seeAlso rdf:resource="&j2se-1_5;JavaxManagementLibrary"/>
		<rdfs:seeAlso rdf:resource="&j2se-1_5;JavaNetLibrary"/>
		<rdfs:seeAlso rdf:resource="&j2se-1_5;JavaUtilLibrary"/>
		<rdfs:comment xml:lang="en">JavaLibrary implementing the javax.management.loading package for j2se-1_5</rdfs:comment>
	</owl:Class>
	<owl:Class rdf:about="&j2se-1_5;OrgOmgStubJavaxManagementRemoteRmiLibrary">
		<rdfs:subClassOf rdf:resource="&java;JavaLibrary"/>
		<rdfs:seeAlso rdf:resource="&j2se-1_5;OrgOmgCORBAPortableLibrary"/>
		<rdfs:seeAlso rdf:resource="&j2se-1_5;JavaxRmiCORBALibrary"/>
		<rdfs:seeAlso rdf:resource="&j2se-1_5;JavaxSecurityAuthLibrary"/>
		<rdfs:seeAlso rdf:resource="&j2se-1_5;JavaRmiLibrary"/>
		<rdfs:seeAlso rdf:resource="&j2se-1_5;JavaLangLibrary"/>
		<rdfs:seeAlso rdf:resource="&j2se-1_5;JavaxManagementRemoteLibrary"/>
		<rdfs:seeAlso rdf:resource="&j2se-1_5;JavaxManagementLibrary"/>
		<rdfs:seeAlso rdf:resource="&j2se-1_5;OrgOmgCORBA_2_3PortableLibrary"/>
		<rdfs:seeAlso rdf:resource="&j2se-1_5;JavaxManagementRemoteRmiLibrary"/>
		<rdfs:seeAlso rdf:resource="&j2se-1_5;OrgOmgCORBALibrary"/>
		<rdfs:seeAlso rdf:resource="&j2se-1_5;JavaUtilLibrary"/>
		<rdfs:comment xml:lang="en">JavaLibrary implementing the org.omg.stub.javax.management.remote.rmi package for j2se-1_5</rdfs:comment>
	</owl:Class>
	<owl:Class rdf:about="&j2se-1_5;JavaxPrintAttributeLibrary">
		<owl:equivalentClass rdf:resource="&j2se-1_4;JavaxPrintAttributeLibrary"/>
		<rdfs:subClassOf rdf:resource="&java;JavaLibrary"/>
		<rdfs:seeAlso rdf:resource="&j2se-1_5;JavaNetLibrary"/>
		<rdfs:seeAlso rdf:resource="&j2se-1_5;JavaIoLibrary"/>
		<rdfs:seeAlso rdf:resource="&j2se-1_5;JavaLangLibrary"/>
		<rdfs:seeAlso rdf:resource="&j2se-1_5;JavaUtilLibrary"/>
		<rdfs:comment xml:lang="en">JavaLibrary implementing the javax.print.attribute package for j2se-1_5</rdfs:comment>
	</owl:Class>
	<owl:Class rdf:about="&j2se-1_5;JavaxActivityLibrary">
		<rdfs:subClassOf rdf:resource="&java;JavaLibrary"/>
		<rdfs:seeAlso rdf:resource="&j2se-1_5;JavaRmiLibrary"/>
		<rdfs:seeAlso rdf:resource="&j2se-1_5;JavaLangLibrary"/>
		<rdfs:comment xml:lang="en">JavaLibrary implementing the javax.activity package for j2se-1_5</rdfs:comment>
	</owl:Class>
	<owl:Class rdf:about="&j2se-1_5;JavaxPrintEventLibrary">
		<owl:equivalentClass rdf:resource="&j2se-1_4;JavaxPrintEventLibrary"/>
		<rdfs:subClassOf rdf:resource="&java;JavaLibrary"/>
		<rdfs:seeAlso rdf:resource="&j2se-1_5;JavaxPrintLibrary"/>
		<rdfs:seeAlso rdf:resource="&j2se-1_5;JavaLangLibrary"/>
		<rdfs:seeAlso rdf:resource="&j2se-1_5;JavaUtilLibrary"/>
		<rdfs:seeAlso rdf:resource="&j2se-1_5;JavaxPrintAttributeLibrary"/>
		<rdfs:comment xml:lang="en">JavaLibrary implementing the javax.print.event package for j2se-1_5</rdfs:comment>
	</owl:Class>
	<owl:Class rdf:about="&j2se-1_5;JavaxManagementRemoteRmiLibrary">
		<rdfs:subClassOf rdf:resource="&java;JavaLibrary"/>
		<rdfs:seeAlso rdf:resource="&j2se-1_5;JavaUtilLibrary"/>
		<rdfs:seeAlso rdf:resource="&j2se-1_5;JavaxSecurityAuthLibrary"/>
		<rdfs:seeAlso rdf:resource="&j2se-1_5;JavaRmiLibrary"/>
		<rdfs:seeAlso rdf:resource="&j2se-1_5;JavaIoLibrary"/>
		<rdfs:seeAlso rdf:resource="&j2se-1_5;JavaLangLibrary"/>
		<rdfs:seeAlso rdf:resource="&j2se-1_5;JavaxManagementRemoteLibrary"/>
		<rdfs:seeAlso rdf:resource="&j2se-1_5;JavaxManagementLibrary"/>
		<rdfs:seeAlso rdf:resource="&j2se-1_5;JavaRmiServerLibrary"/>
		<rdfs:comment xml:lang="en">JavaLibrary implementing the javax.management.remote.rmi package for j2se-1_5</rdfs:comment>
	</owl:Class>
	<owl:Class rdf:about="&j2se-1_5;JavaxImageioPluginsJpegLibrary">
		<owl:equivalentClass rdf:resource="&j2se-1_4;JavaxImageioPluginsJpegLibrary"/>
		<rdfs:subClassOf rdf:resource="&java;JavaLibrary"/>
		<rdfs:seeAlso rdf:resource="&j2se-1_5;JavaxImageioLibrary"/>
		<rdfs:seeAlso rdf:resource="&j2se-1_5;JavaLangLibrary"/>
		<rdfs:seeAlso rdf:resource="&j2se-1_5;JavaUtilLibrary"/>
		<rdfs:comment xml:lang="en">JavaLibrary implementing the javax.imageio.plugins.jpeg package for j2se-1_5</rdfs:comment>
	</owl:Class>
	<owl:Class rdf:about="&j2se-1_5;JavaUtilLibrary">
		<rdfs:subClassOf rdf:resource="&j2se-1_4;JavaUtilLibrary"/>
		<rdfs:seeAlso rdf:resource="&j2se-1_5;JavaUtilRegexLibrary"/>
		<rdfs:seeAlso rdf:resource="&j2se-1_5;JavaSecurityLibrary"/>
		<rdfs:seeAlso rdf:resource="&j2se-1_5;JavaIoLibrary"/>
		<rdfs:seeAlso rdf:resource="&j2se-1_5;JavaLangLibrary"/>
		<rdfs:seeAlso rdf:resource="&j2se-1_5;JavaNioChannelsLibrary"/>
		<rdfs:seeAlso rdf:resource="&j2se-1_5;JavaMathLibrary"/>
		<rdfs:comment xml:lang="en">JavaLibrary implementing the java.util package for j2se-1_5</rdfs:comment>
	</owl:Class>
	<owl:Class rdf:about="&j2se-1_5;OrgOmgDynamicAnyLibrary">
		<rdfs:subClassOf rdf:resource="&j2se-1_4;OrgOmgDynamicAnyLibrary"/>
		<rdfs:seeAlso rdf:resource="&j2se-1_5;OrgOmgCORBAPortableLibrary"/>
		<rdfs:seeAlso rdf:resource="&j2se-1_5;JavaIoLibrary"/>
		<rdfs:seeAlso rdf:resource="&j2se-1_5;JavaLangLibrary"/>
		<rdfs:seeAlso rdf:resource="&j2se-1_5;OrgOmgCORBALibrary"/>
		<rdfs:comment xml:lang="en">JavaLibrary implementing the org.omg.DynamicAny package for j2se-1_5</rdfs:comment>
	</owl:Class>
	<owl:Class rdf:about="&j2se-1_5;JavaxSwingFilechooserLibrary">
		<owl:equivalentClass rdf:resource="&j2se-1_4;JavaxSwingFilechooserLibrary"/>
		<rdfs:subClassOf rdf:resource="&java;JavaLibrary"/>
		<rdfs:seeAlso rdf:resource="&j2se-1_5;JavaxSwingLibrary"/>
		<rdfs:seeAlso rdf:resource="&j2se-1_5;JavaIoLibrary"/>
		<rdfs:seeAlso rdf:resource="&j2se-1_5;JavaLangLibrary"/>
		<rdfs:comment xml:lang="en">JavaLibrary implementing the javax.swing.filechooser package for j2se-1_5</rdfs:comment>
	</owl:Class>
	<owl:Class rdf:about="&j2se-1_5;JavaNioChannelsSpiLibrary">
		<rdfs:subClassOf rdf:resource="&j2se-1_4;JavaNioChannelsSpiLibrary"/>
		<rdfs:seeAlso rdf:resource="&j2se-1_5;JavaNioChannelsLibrary"/>
		<rdfs:seeAlso rdf:resource="&j2se-1_5;JavaLangLibrary"/>
		<rdfs:seeAlso rdf:resource="&j2se-1_5;JavaUtilLibrary"/>
		<rdfs:comment xml:lang="en">JavaLibrary implementing the java.nio.channels.spi package for j2se-1_5</rdfs:comment>
	</owl:Class>
	<owl:Class rdf:about="&j2se-1_5;OrgOmgCosNamingLibrary">
		<rdfs:subClassOf rdf:resource="&j2se-1_4;OrgOmgCosNamingLibrary"/>
		<rdfs:seeAlso rdf:resource="&j2se-1_5;OrgOmgCORBAPortableLibrary"/>
		<rdfs:seeAlso rdf:resource="&j2se-1_5;JavaLangLibrary"/>
		<rdfs:seeAlso rdf:resource="&j2se-1_5;OrgOmgPortableServerLibrary"/>
		<rdfs:seeAlso rdf:resource="&j2se-1_5;OrgOmgCORBALibrary"/>
		<rdfs:comment xml:lang="en">JavaLibrary implementing the org.omg.CosNaming package for j2se-1_5</rdfs:comment>
	</owl:Class>
	<owl:Class rdf:about="&j2se-1_5;OrgXmlSaxExtLibrary">
		<rdfs:subClassOf rdf:resource="&j2se-1_4;OrgXmlSaxExtLibrary"/>
		<rdfs:seeAlso rdf:resource="&j2se-1_5;JavaLangLibrary"/>
		<rdfs:seeAlso rdf:resource="&j2se-1_5;OrgXmlSaxLibrary"/>
		<rdfs:seeAlso rdf:resource="&j2se-1_5;OrgXmlSaxHelpersLibrary"/>
		<rdfs:comment xml:lang="en">JavaLibrary implementing the org.xml.sax.ext package for j2se-1_5</rdfs:comment>
	</owl:Class>
	<owl:Class rdf:about="&j2se-1_5;JavaxTransactionLibrary">
		<owl:equivalentClass rdf:resource="&j2se-1_4;JavaxTransactionLibrary"/>
		<rdfs:subClassOf rdf:resource="&java;JavaLibrary"/>
		<rdfs:seeAlso rdf:resource="&j2se-1_5;JavaRmiLibrary"/>
		<rdfs:seeAlso rdf:resource="&j2se-1_5;JavaLangLibrary"/>
		<rdfs:comment xml:lang="en">JavaLibrary implementing the javax.transaction package for j2se-1_5</rdfs:comment>
	</owl:Class>
	<owl:Class rdf:about="&j2se-1_5;JavaxPrintAttributeStandardLibrary">
		<rdfs:subClassOf rdf:resource="&j2se-1_4;JavaxPrintAttributeStandardLibrary"/>
		<rdfs:seeAlso rdf:resource="&j2se-1_5;JavaxPrintAttributeLibrary"/>
		<rdfs:seeAlso rdf:resource="&j2se-1_5;JavaUtilLibrary"/>
		<rdfs:seeAlso rdf:resource="&j2se-1_5;JavaLangLibrary"/>
		<rdfs:seeAlso rdf:resource="&j2se-1_5;JavaNetLibrary"/>
		<rdfs:comment xml:lang="en">JavaLibrary implementing the javax.print.attribute.standard package for j2se-1_5</rdfs:comment>
	</owl:Class>
	<owl:Class rdf:about="&j2se-1_5;JavaxAccessibilityLibrary">
		<rdfs:subClassOf rdf:resource="&j2se-1_4;JavaxAccessibilityLibrary"/>
		<rdfs:seeAlso rdf:resource="&j2se-1_5;JavaBeansLibrary"/>
		<rdfs:seeAlso rdf:resource="&j2se-1_5;JavaIoLibrary"/>
		<rdfs:seeAlso rdf:resource="&j2se-1_5;JavaxSwingTextLibrary"/>
		<rdfs:seeAlso rdf:resource="&j2se-1_5;JavaLangLibrary"/>
		<rdfs:seeAlso rdf:resource="&j2se-1_5;JavaAwtEventLibrary"/>
		<rdfs:seeAlso rdf:resource="&j2se-1_5;JavaAwtDatatransferLibrary"/>
		<rdfs:seeAlso rdf:resource="&j2se-1_5;JavaAwtLibrary"/>
		<rdfs:seeAlso rdf:resource="&j2se-1_5;JavaUtilLibrary"/>
		<rdfs:comment xml:lang="en">JavaLibrary implementing the javax.accessibility package for j2se-1_5</rdfs:comment>
	</owl:Class>
	<owl:Class rdf:about="&j2se-1_5;JavaxImageioSpiLibrary">
		<owl:equivalentClass rdf:resource="&j2se-1_4;JavaxImageioSpiLibrary"/>
		<rdfs:subClassOf rdf:resource="&java;JavaLibrary"/>
		<rdfs:seeAlso rdf:resource="&j2se-1_5;JavaAwtImageLibrary"/>
		<rdfs:seeAlso rdf:resource="&j2se-1_5;JavaxImageioLibrary"/>
		<rdfs:seeAlso rdf:resource="&j2se-1_5;JavaxImageioMetadataLibrary"/>
		<rdfs:seeAlso rdf:resource="&j2se-1_5;JavaIoLibrary"/>
		<rdfs:seeAlso rdf:resource="&j2se-1_5;JavaLangLibrary"/>
		<rdfs:seeAlso rdf:resource="&j2se-1_5;JavaUtilLibrary"/>
		<rdfs:seeAlso rdf:resource="&j2se-1_5;JavaxImageioStreamLibrary"/>
		<rdfs:comment xml:lang="en">JavaLibrary implementing the javax.imageio.spi package for j2se-1_5</rdfs:comment>
	</owl:Class>
	<owl:Class rdf:about="&j2se-1_5;JavaBeansLibrary">
		<rdfs:subClassOf rdf:resource="&j2se-1_4;JavaBeansLibrary"/>
		<rdfs:seeAlso rdf:resource="&j2se-1_5;JavaLangReflectLibrary"/>
		<rdfs:seeAlso rdf:resource="&j2se-1_5;JavaAppletLibrary"/>
		<rdfs:seeAlso rdf:resource="&j2se-1_5;JavaIoLibrary"/>
		<rdfs:seeAlso rdf:resource="&j2se-1_5;JavaBeansBeancontextLibrary"/>
		<rdfs:seeAlso rdf:resource="&j2se-1_5;JavaLangLibrary"/>
		<rdfs:seeAlso rdf:resource="&j2se-1_5;JavaAwtLibrary"/>
		<rdfs:seeAlso rdf:resource="&j2se-1_5;JavaUtilLibrary"/>
		<rdfs:comment xml:lang="en">JavaLibrary implementing the java.beans package for j2se-1_5</rdfs:comment>
	</owl:Class>
	<owl:Class rdf:about="&j2se-1_5;JavaxImageioMetadataLibrary">
		<rdfs:subClassOf rdf:resource="&j2se-1_4;JavaxImageioMetadataLibrary"/>
		<rdfs:seeAlso rdf:resource="&j2se-1_5;JavaxImageioLibrary"/>
		<rdfs:seeAlso rdf:resource="&j2se-1_5;JavaLangLibrary"/>
		<rdfs:seeAlso rdf:resource="&j2se-1_5;JavaUtilLibrary"/>
		<rdfs:seeAlso rdf:resource="&j2se-1_5;OrgW3cDomLibrary"/>
		<rdfs:comment xml:lang="en">JavaLibrary implementing the javax.imageio.metadata package for j2se-1_5</rdfs:comment>
	</owl:Class>
	<owl:Class rdf:about="&j2se-1_5;JavaRmiRegistryLibrary">
		<owl:equivalentClass rdf:resource="&j2se-1_4;JavaRmiRegistryLibrary"/>
		<rdfs:subClassOf rdf:resource="&java;JavaLibrary"/>
		<rdfs:seeAlso rdf:resource="&j2se-1_5;JavaRmiServerLibrary"/>
		<rdfs:seeAlso rdf:resource="&j2se-1_5;JavaRmiLibrary"/>
		<rdfs:seeAlso rdf:resource="&j2se-1_5;JavaLangLibrary"/>
		<rdfs:comment xml:lang="en">JavaLibrary implementing the java.rmi.registry package for j2se-1_5</rdfs:comment>
	</owl:Class>
	<owl:Class rdf:about="&j2se-1_5;JavaLangLibrary">
		<rdfs:subClassOf rdf:resource="&java;JavaLibrary"/>
		<rdfs:seeAlso rdf:resource="&j2se-1_5;JavaLangReflectLibrary"/>
		<rdfs:seeAlso rdf:resource="&j2se-1_5;JavaLangAnnotationLibrary"/>
		<rdfs:seeAlso rdf:resource="&j2se-1_5;JavaSecurityLibrary"/>
		<rdfs:seeAlso rdf:resource="&j2se-1_5;JavaUtilLibrary"/>
		<rdfs:seeAlso rdf:resource="&j2se-1_5;JavaIoLibrary"/>
		<rdfs:seeAlso rdf:resource="&j2se-1_5;JavaNioLibrary"/>
		<rdfs:seeAlso rdf:resource="&j2se-1_5;JavaNetLibrary"/>
		<rdfs:seeAlso rdf:resource="&j2se-1_5;JavaNioChannelsLibrary"/>
		<rdfs:comment xml:lang="en">JavaLibrary implementing the java.lang package for j2se-1_5</rdfs:comment>
	</owl:Class>
	<owl:Class rdf:about="&j2se-1_5;JavaxSwingEventLibrary">
		<rdfs:subClassOf rdf:resource="&j2se-1_4;JavaxSwingEventLibrary"/>
		<rdfs:seeAlso rdf:resource="&j2se-1_5;JavaxSwingTableLibrary"/>
		<rdfs:seeAlso rdf:resource="&j2se-1_5;JavaUtilLibrary"/>
		<rdfs:seeAlso rdf:resource="&j2se-1_5;JavaxSwingLibrary"/>
		<rdfs:seeAlso rdf:resource="&j2se-1_5;JavaBeansLibrary"/>
		<rdfs:seeAlso rdf:resource="&j2se-1_5;JavaIoLibrary"/>
		<rdfs:seeAlso rdf:resource="&j2se-1_5;JavaLangLibrary"/>
		<rdfs:seeAlso rdf:resource="&j2se-1_5;JavaxSwingTextLibrary"/>
		<rdfs:seeAlso rdf:resource="&j2se-1_5;JavaAwtEventLibrary"/>
		<rdfs:seeAlso rdf:resource="&j2se-1_5;JavaAwtLibrary"/>
		<rdfs:seeAlso rdf:resource="&j2se-1_5;JavaNetLibrary"/>
		<rdfs:seeAlso rdf:resource="&j2se-1_5;JavaxSwingUndoLibrary"/>
		<rdfs:seeAlso rdf:resource="&j2se-1_5;JavaxSwingTreeLibrary"/>
		<rdfs:comment xml:lang="en">JavaLibrary implementing the javax.swing.event package for j2se-1_5</rdfs:comment>
	</owl:Class>
	<owl:Class rdf:about="&j2se-1_5;JavaxSecurityAuthCallbackLibrary">
		<owl:equivalentClass rdf:resource="&j2se-1_4;JavaxSecurityAuthCallbackLibrary"/>
		<rdfs:subClassOf rdf:resource="&java;JavaLibrary"/>
		<rdfs:seeAlso rdf:resource="&j2se-1_5;JavaIoLibrary"/>
		<rdfs:seeAlso rdf:resource="&j2se-1_5;JavaLangLibrary"/>
		<rdfs:seeAlso rdf:resource="&j2se-1_5;JavaUtilLibrary"/>
		<rdfs:comment xml:lang="en">JavaLibrary implementing the javax.security.auth.callback package for j2se-1_5</rdfs:comment>
	</owl:Class>
	<owl:Class rdf:about="&j2se-1_5;OrgW3cDomBootstrapLibrary">
		<rdfs:subClassOf rdf:resource="&java;JavaLibrary"/>
		<rdfs:seeAlso rdf:resource="&j2se-1_5;JavaLangLibrary"/>
		<rdfs:seeAlso rdf:resource="&j2se-1_5;OrgW3cDomLibrary"/>
		<rdfs:comment xml:lang="en">JavaLibrary implementing the org.w3c.dom.bootstrap package for j2se-1_5</rdfs:comment>
	</owl:Class>
	<owl:Class rdf:about="&j2se-1_5;OrgOmgCosNamingNamingContextPackageLibrary">
		<owl:equivalentClass rdf:resource="&j2se-1_4;OrgOmgCosNamingNamingContextPackageLibrary"/>
		<rdfs:subClassOf rdf:resource="&java;JavaLibrary"/>
		<rdfs:seeAlso rdf:resource="&j2se-1_5;OrgOmgCosNamingLibrary"/>
		<rdfs:seeAlso rdf:resource="&j2se-1_5;OrgOmgCORBAPortableLibrary"/>
		<rdfs:seeAlso rdf:resource="&j2se-1_5;OrgOmgCORBALibrary"/>
		<rdfs:seeAlso rdf:resource="&j2se-1_5;JavaLangLibrary"/>
		<rdfs:comment xml:lang="en">JavaLibrary implementing the org.omg.CosNaming.NamingContextPackage package for j2se-1_5</rdfs:comment>
	</owl:Class>
	<owl:Class rdf:about="&j2se-1_5;JavaTextLibrary">
		<rdfs:subClassOf rdf:resource="&java;JavaLibrary"/>
		<rdfs:seeAlso rdf:resource="&j2se-1_5;JavaIoLibrary"/>
		<rdfs:seeAlso rdf:resource="&j2se-1_5;JavaLangLibrary"/>
		<rdfs:seeAlso rdf:resource="&j2se-1_5;JavaUtilLibrary"/>
		<rdfs:comment xml:lang="en">JavaLibrary implementing the java.text package for j2se-1_5</rdfs:comment>
	</owl:Class>
	<owl:Class rdf:about="&j2se-1_5;OrgW3cDomLibrary">
		<rdfs:subClassOf rdf:resource="&j2se-1_4;OrgW3cDomLibrary"/>
		<rdfs:seeAlso rdf:resource="&j2se-1_5;JavaLangLibrary"/>
		<rdfs:comment xml:lang="en">JavaLibrary implementing the org.w3c.dom package for j2se-1_5</rdfs:comment>
	</owl:Class>
	<owl:Class rdf:about="&j2se-1_5;JavaxXmlLibrary">
		<rdfs:subClassOf rdf:resource="&java;JavaLibrary"/>
		<rdfs:seeAlso rdf:resource="&j2se-1_5;JavaLangLibrary"/>
		<rdfs:comment xml:lang="en">JavaLibrary implementing the javax.xml package for j2se-1_5</rdfs:comment>
	</owl:Class>
	<owl:Class rdf:about="&j2se-1_5;JavaNioCharsetLibrary">
		<rdfs:subClassOf rdf:resource="&j2se-1_4;JavaNioCharsetLibrary"/>
		<rdfs:seeAlso rdf:resource="&j2se-1_5;JavaIoLibrary"/>
		<rdfs:seeAlso rdf:resource="&j2se-1_5;JavaNioLibrary"/>
		<rdfs:seeAlso rdf:resource="&j2se-1_5;JavaLangLibrary"/>
		<rdfs:seeAlso rdf:resource="&j2se-1_5;JavaUtilLibrary"/>
		<rdfs:comment xml:lang="en">JavaLibrary implementing the java.nio.charset package for j2se-1_5</rdfs:comment>
	</owl:Class>
	<owl:Class rdf:about="&j2se-1_5;OrgOmgDynamicAnyDynAnyFactoryPackageLibrary">
		<owl:equivalentClass rdf:resource="&j2se-1_4;OrgOmgDynamicAnyDynAnyFactoryPackageLibrary"/>
		<rdfs:subClassOf rdf:resource="&java;JavaLibrary"/>
		<rdfs:seeAlso rdf:resource="&j2se-1_5;OrgOmgCORBAPortableLibrary"/>
		<rdfs:seeAlso rdf:resource="&j2se-1_5;OrgOmgCORBALibrary"/>
		<rdfs:seeAlso rdf:resource="&j2se-1_5;JavaLangLibrary"/>
		<rdfs:comment xml:lang="en">JavaLibrary implementing the org.omg.DynamicAny.DynAnyFactoryPackage package for j2se-1_5</rdfs:comment>
	</owl:Class>
	<owl:Class rdf:about="&j2se-1_5;OrgOmgSendingContextLibrary">
		<owl:equivalentClass rdf:resource="&j2se-1_4;OrgOmgSendingContextLibrary"/>
		<rdfs:subClassOf rdf:resource="&java;JavaLibrary"/>
		<rdfs:seeAlso rdf:resource="&j2se-1_5;OrgOmgCORBAPortableLibrary"/>
		<rdfs:seeAlso rdf:resource="&j2se-1_5;OrgOmgCORBALibrary"/>
		<rdfs:comment xml:lang="en">JavaLibrary implementing the org.omg.SendingContext package for j2se-1_5</rdfs:comment>
	</owl:Class>
	<owl:Class rdf:about="&j2se-1_5;OrgOmgPortableInterceptorLibrary">
		<rdfs:subClassOf rdf:resource="&j2se-1_4;OrgOmgPortableInterceptorLibrary"/>
		<rdfs:seeAlso rdf:resource="&j2se-1_5;OrgOmgCORBAPortableLibrary"/>
		<rdfs:seeAlso rdf:resource="&j2se-1_5;JavaLangLibrary"/>
		<rdfs:seeAlso rdf:resource="&j2se-1_5;OrgOmgIOPLibrary"/>
		<rdfs:seeAlso rdf:resource="&j2se-1_5;OrgOmgCORBALibrary"/>
		<rdfs:comment xml:lang="en">JavaLibrary implementing the org.omg.PortableInterceptor package for j2se-1_5</rdfs:comment>
	</owl:Class>
	<owl:Class rdf:about="&j2se-1_5;JavaxNamingLdapLibrary">
		<rdfs:subClassOf rdf:resource="&j2se-1_4;JavaxNamingLdapLibrary"/>
		<rdfs:seeAlso rdf:resource="&j2se-1_5;JavaIoLibrary"/>
		<rdfs:seeAlso rdf:resource="&j2se-1_5;JavaLangLibrary"/>
		<rdfs:seeAlso rdf:resource="&j2se-1_5;JavaxNamingDirectoryLibrary"/>
		<rdfs:seeAlso rdf:resource="&j2se-1_5;JavaxNamingLibrary"/>
		<rdfs:seeAlso rdf:resource="&j2se-1_5;JavaUtilLibrary"/>
		<rdfs:seeAlso rdf:resource="&j2se-1_5;JavaxNamingEventLibrary"/>
		<rdfs:comment xml:lang="en">JavaLibrary implementing the javax.naming.ldap package for j2se-1_5</rdfs:comment>
	</owl:Class>
	<owl:Class rdf:about="&j2se-1_5;JavaLangReflectLibrary">
		<rdfs:subClassOf rdf:resource="&j2se-1_4;JavaLangReflectLibrary"/>
		<rdfs:seeAlso rdf:resource="&j2se-1_5;JavaLangAnnotationLibrary"/>
		<rdfs:seeAlso rdf:resource="&j2se-1_5;JavaSecurityLibrary"/>
		<rdfs:seeAlso rdf:resource="&j2se-1_5;JavaIoLibrary"/>
		<rdfs:seeAlso rdf:resource="&j2se-1_5;JavaLangLibrary"/>
		<rdfs:comment xml:lang="en">JavaLibrary implementing the java.lang.reflect package for j2se-1_5</rdfs:comment>
	</owl:Class>
	<owl:Class rdf:about="&j2se-1_5;JavaxSwingTextHtmlLibrary">
		<rdfs:subClassOf rdf:resource="&j2se-1_4;JavaxSwingTextHtmlLibrary"/>
		<rdfs:seeAlso rdf:resource="&j2se-1_5;JavaUtilLibrary"/>
		<rdfs:seeAlso rdf:resource="&j2se-1_5;JavaxAccessibilityLibrary"/>
		<rdfs:seeAlso rdf:resource="&j2se-1_5;JavaLangLibrary"/>
		<rdfs:seeAlso rdf:resource="&j2se-1_5;JavaxSwingEventLibrary"/>
		<rdfs:seeAlso rdf:resource="&j2se-1_5;JavaAwtLibrary"/>
		<rdfs:seeAlso rdf:resource="&j2se-1_5;JavaxSwingLibrary"/>
		<rdfs:seeAlso rdf:resource="&j2se-1_5;JavaIoLibrary"/>
		<rdfs:seeAlso rdf:resource="&j2se-1_5;JavaxSwingTextLibrary"/>
		<rdfs:seeAlso rdf:resource="&j2se-1_5;JavaAwtEventLibrary"/>
		<rdfs:seeAlso rdf:resource="&j2se-1_5;JavaNetLibrary"/>
		<rdfs:comment xml:lang="en">JavaLibrary implementing the javax.swing.text.html package for j2se-1_5</rdfs:comment>
	</owl:Class>
	<owl:Class rdf:about="&j2se-1_5;JavaxXmlXpathLibrary">
		<rdfs:subClassOf rdf:resource="&java;JavaLibrary"/>
		<rdfs:seeAlso rdf:resource="&j2se-1_5;JavaxXmlNamespaceLibrary"/>
		<rdfs:seeAlso rdf:resource="&j2se-1_5;JavaIoLibrary"/>
		<rdfs:seeAlso rdf:resource="&j2se-1_5;JavaLangLibrary"/>
		<rdfs:seeAlso rdf:resource="&j2se-1_5;JavaUtilLibrary"/>
		<rdfs:seeAlso rdf:resource="&j2se-1_5;OrgXmlSaxLibrary"/>
		<rdfs:comment xml:lang="en">JavaLibrary implementing the javax.xml.xpath package for j2se-1_5</rdfs:comment>
	</owl:Class>
	<owl:Class rdf:about="&j2se-1_5;JavaxSoundMidiSpiLibrary">
		<owl:equivalentClass rdf:resource="&j2se-1_4;JavaxSoundMidiSpiLibrary"/>
		<rdfs:subClassOf rdf:resource="&java;JavaLibrary"/>
		<rdfs:seeAlso rdf:resource="&j2se-1_5;JavaNetLibrary"/>
		<rdfs:seeAlso rdf:resource="&j2se-1_5;JavaIoLibrary"/>
		<rdfs:seeAlso rdf:resource="&j2se-1_5;JavaLangLibrary"/>
		<rdfs:seeAlso rdf:resource="&j2se-1_5;JavaxSoundMidiLibrary"/>
		<rdfs:comment xml:lang="en">JavaLibrary implementing the javax.sound.midi.spi package for j2se-1_5</rdfs:comment>
	</owl:Class>
	<owl:Class rdf:about="&j2se-1_5;JavaxSecurityAuthLoginLibrary">
		<rdfs:subClassOf rdf:resource="&j2se-1_4;JavaxSecurityAuthLoginLibrary"/>
		<rdfs:seeAlso rdf:resource="&j2se-1_5;JavaSecurityLibrary"/>
		<rdfs:seeAlso rdf:resource="&j2se-1_5;JavaxSecurityAuthLibrary"/>
		<rdfs:seeAlso rdf:resource="&j2se-1_5;JavaLangLibrary"/>
		<rdfs:seeAlso rdf:resource="&j2se-1_5;JavaUtilLibrary"/>
		<rdfs:seeAlso rdf:resource="&j2se-1_5;JavaxSecurityAuthCallbackLibrary"/>
		<rdfs:comment xml:lang="en">JavaLibrary implementing the javax.security.auth.login package for j2se-1_5</rdfs:comment>
	</owl:Class>
	<owl:Class rdf:about="&j2se-1_5;OrgOmgPortableServerPortableLibrary">
		<owl:equivalentClass rdf:resource="&j2se-1_4;OrgOmgPortableServerPortableLibrary"/>
		<rdfs:subClassOf rdf:resource="&java;JavaLibrary"/>
		<rdfs:seeAlso rdf:resource="&j2se-1_5;OrgOmgPortableServerLibrary"/>
		<rdfs:seeAlso rdf:resource="&j2se-1_5;OrgOmgCORBALibrary"/>
		<rdfs:seeAlso rdf:resource="&j2se-1_5;JavaLangLibrary"/>
		<rdfs:comment xml:lang="en">JavaLibrary implementing the org.omg.PortableServer.portable package for j2se-1_5</rdfs:comment>
	</owl:Class>
	<owl:Class rdf:about="&j2se-1_5;OrgOmgCORBA_2_3Library">
		<owl:equivalentClass rdf:resource="&j2se-1_4;OrgOmgCORBA_2_3Library"/>
		<rdfs:subClassOf rdf:resource="&java;JavaLibrary"/>
		<rdfs:seeAlso rdf:resource="&j2se-1_5;OrgOmgCORBAPortableLibrary"/>
		<rdfs:seeAlso rdf:resource="&j2se-1_5;OrgOmgCORBALibrary"/>
		<rdfs:seeAlso rdf:resource="&j2se-1_5;JavaLangLibrary"/>
		<rdfs:comment xml:lang="en">JavaLibrary implementing the org.omg.CORBA_2_3 package for j2se-1_5</rdfs:comment>
	</owl:Class>
	<owl:Class rdf:about="&j2se-1_5;JavaxSwingTableLibrary">
		<rdfs:subClassOf rdf:resource="&j2se-1_4;JavaxSwingTableLibrary"/>
		<rdfs:seeAlso rdf:resource="&j2se-1_5;JavaxSwingPlafLibrary"/>
		<rdfs:seeAlso rdf:resource="&j2se-1_5;JavaUtilLibrary"/>
		<rdfs:seeAlso rdf:resource="&j2se-1_5;JavaxSwingBorderLibrary"/>
		<rdfs:seeAlso rdf:resource="&j2se-1_5;JavaxSwingLibrary"/>
		<rdfs:seeAlso rdf:resource="&j2se-1_5;JavaxAccessibilityLibrary"/>
		<rdfs:seeAlso rdf:resource="&j2se-1_5;JavaBeansLibrary"/>
		<rdfs:seeAlso rdf:resource="&j2se-1_5;JavaIoLibrary"/>
		<rdfs:seeAlso rdf:resource="&j2se-1_5;JavaAwtEventLibrary"/>
		<rdfs:seeAlso rdf:resource="&j2se-1_5;JavaLangLibrary"/>
		<rdfs:seeAlso rdf:resource="&j2se-1_5;JavaxSwingEventLibrary"/>
		<rdfs:seeAlso rdf:resource="&j2se-1_5;JavaAwtLibrary"/>
		<rdfs:comment xml:lang="en">JavaLibrary implementing the javax.swing.table package for j2se-1_5</rdfs:comment>
	</owl:Class>
	<owl:Class rdf:about="&j2se-1_5;JavaxNamingDirectoryLibrary">
		<rdfs:subClassOf rdf:resource="&j2se-1_4;JavaxNamingDirectoryLibrary"/>
		<rdfs:seeAlso rdf:resource="&j2se-1_5;JavaIoLibrary"/>
		<rdfs:seeAlso rdf:resource="&j2se-1_5;JavaLangLibrary"/>
		<rdfs:seeAlso rdf:resource="&j2se-1_5;JavaxNamingLibrary"/>
		<rdfs:seeAlso rdf:resource="&j2se-1_5;JavaUtilLibrary"/>
		<rdfs:comment xml:lang="en">JavaLibrary implementing the javax.naming.directory package for j2se-1_5</rdfs:comment>
	</owl:Class>
	<owl:Class rdf:about="&j2se-1_5;JavaxSwingPlafLibrary">
		<rdfs:subClassOf rdf:resource="&j2se-1_4;JavaxSwingPlafLibrary"/>
		<rdfs:seeAlso rdf:resource="&j2se-1_5;JavaxSwingFilechooserLibrary"/>
		<rdfs:seeAlso rdf:resource="&j2se-1_5;JavaxSwingBorderLibrary"/>
		<rdfs:seeAlso rdf:resource="&j2se-1_5;JavaxSwingLibrary"/>
		<rdfs:seeAlso rdf:resource="&j2se-1_5;JavaxAccessibilityLibrary"/>
		<rdfs:seeAlso rdf:resource="&j2se-1_5;JavaIoLibrary"/>
		<rdfs:seeAlso rdf:resource="&j2se-1_5;JavaLangLibrary"/>
		<rdfs:seeAlso rdf:resource="&j2se-1_5;JavaAwtEventLibrary"/>
		<rdfs:seeAlso rdf:resource="&j2se-1_5;JavaxSwingTextLibrary"/>
		<rdfs:seeAlso rdf:resource="&j2se-1_5;JavaAwtLibrary"/>
		<rdfs:seeAlso rdf:resource="&j2se-1_5;JavaxSwingTreeLibrary"/>
		<rdfs:comment xml:lang="en">JavaLibrary implementing the javax.swing.plaf package for j2se-1_5</rdfs:comment>
	</owl:Class>
	<owl:Class rdf:about="&j2se-1_5;OrgOmgStubJavaRmiLibrary">
		<owl:equivalentClass rdf:resource="&j2se-1_4;OrgOmgStubJavaRmiLibrary"/>
		<rdfs:subClassOf rdf:resource="&java;JavaLibrary"/>
		<rdfs:seeAlso rdf:resource="&j2se-1_5;JavaxRmiCORBALibrary"/>
		<rdfs:seeAlso rdf:resource="&j2se-1_5;JavaRmiLibrary"/>
		<rdfs:comment xml:lang="en">JavaLibrary implementing the org.omg.stub.java.rmi package for j2se-1_5</rdfs:comment>
	</owl:Class>
	<owl:Class rdf:about="&j2se-1_5;JavaxCryptoLibrary">
		<owl:equivalentClass rdf:resource="&j2se-1_4;JavaxCryptoLibrary"/>
		<rdfs:subClassOf rdf:resource="&java;JavaLibrary"/>
		<rdfs:comment xml:lang="en">JavaLibrary implementing the javax.crypto package for j2se-1_5</rdfs:comment>
	</owl:Class>
	<owl:Class rdf:about="&j2se-1_5;OrgW3cDomViewsLibrary">
		<owl:equivalentClass rdf:resource="&j2se-1_4;OrgW3cDomViewsLibrary"/>
		<rdfs:subClassOf rdf:resource="&java;JavaLibrary"/>
		<rdfs:comment xml:lang="en">JavaLibrary implementing the org.w3c.dom.views package for j2se-1_5</rdfs:comment>
	</owl:Class>
	<owl:Class rdf:about="&j2se-1_5;JavaxSwingPlafSynthLibrary">
		<rdfs:subClassOf rdf:resource="&java;JavaLibrary"/>
		<rdfs:seeAlso rdf:resource="&j2se-1_5;JavaxSwingLibrary"/>
		<rdfs:seeAlso rdf:resource="&j2se-1_5;JavaIoLibrary"/>
		<rdfs:seeAlso rdf:resource="&j2se-1_5;JavaAwtEventLibrary"/>
		<rdfs:seeAlso rdf:resource="&j2se-1_5;JavaLangLibrary"/>
		<rdfs:seeAlso rdf:resource="&j2se-1_5;JavaxSwingPlafLibrary"/>
		<rdfs:seeAlso rdf:resource="&j2se-1_5;JavaAwtLibrary"/>
		<rdfs:seeAlso rdf:resource="&j2se-1_5;JavaxSwingPlafBasicLibrary"/>
		<rdfs:comment xml:lang="en">JavaLibrary implementing the javax.swing.plaf.synth package for j2se-1_5</rdfs:comment>
	</owl:Class>
	<owl:Class rdf:about="&j2se-1_5;JavaLangManagementLibrary">
		<rdfs:subClassOf rdf:resource="&java;JavaLibrary"/>
		<rdfs:seeAlso rdf:resource="&j2se-1_5;JavaxManagementLibrary"/>
		<rdfs:seeAlso rdf:resource="&j2se-1_5;JavaSecurityLibrary"/>
		<rdfs:seeAlso rdf:resource="&j2se-1_5;JavaxManagementOpenmbeanLibrary"/>
		<rdfs:seeAlso rdf:resource="&j2se-1_5;JavaLangLibrary"/>
		<rdfs:seeAlso rdf:resource="&j2se-1_5;JavaUtilLibrary"/>
		<rdfs:comment xml:lang="en">JavaLibrary implementing the java.lang.management package for j2se-1_5</rdfs:comment>
	</owl:Class>
	<owl:Class rdf:about="&j2se-1_5;JavaxSwingBorderLibrary">
		<owl:equivalentClass rdf:resource="&j2se-1_4;JavaxSwingBorderLibrary"/>
		<rdfs:subClassOf rdf:resource="&java;JavaLibrary"/>
		<rdfs:seeAlso rdf:resource="&j2se-1_5;JavaAwtLibrary"/>
		<rdfs:seeAlso rdf:resource="&j2se-1_5;JavaxSwingLibrary"/>
		<rdfs:seeAlso rdf:resource="&j2se-1_5;JavaIoLibrary"/>
		<rdfs:seeAlso rdf:resource="&j2se-1_5;JavaLangLibrary"/>
		<rdfs:comment xml:lang="en">JavaLibrary implementing the javax.swing.border package for j2se-1_5</rdfs:comment>
	</owl:Class>
	<owl:Class rdf:about="&j2se-1_5;OrgW3cDomRangesLibrary">
		<rdfs:subClassOf rdf:resource="&java;JavaLibrary"/>
		<rdfs:seeAlso rdf:resource="&j2se-1_5;JavaLangLibrary"/>
		<rdfs:seeAlso rdf:resource="&j2se-1_5;OrgW3cDomLibrary"/>
		<rdfs:comment xml:lang="en">JavaLibrary implementing the org.w3c.dom.ranges package for j2se-1_5</rdfs:comment>
	</owl:Class>
	<owl:Class rdf:about="&j2se-1_5;JavaxSecurityAuthKerberosLibrary">
		<owl:equivalentClass rdf:resource="&j2se-1_4;JavaxSecurityAuthKerberosLibrary"/>
		<rdfs:subClassOf rdf:resource="&java;JavaLibrary"/>
		<rdfs:seeAlso rdf:resource="&j2se-1_5;JavaSecurityLibrary"/>
		<rdfs:seeAlso rdf:resource="&j2se-1_5;JavaxCryptoLibrary"/>
		<rdfs:seeAlso rdf:resource="&j2se-1_5;JavaxSecurityAuthLibrary"/>
		<rdfs:seeAlso rdf:resource="&j2se-1_5;JavaIoLibrary"/>
		<rdfs:seeAlso rdf:resource="&j2se-1_5;JavaLangLibrary"/>
		<rdfs:seeAlso rdf:resource="&j2se-1_5;JavaUtilLibrary"/>
		<rdfs:comment xml:lang="en">JavaLibrary implementing the javax.security.auth.kerberos package for j2se-1_5</rdfs:comment>
	</owl:Class>
	<owl:Class rdf:about="&j2se-1_5;JavaxSwingLibrary">
		<rdfs:subClassOf rdf:resource="&j2se-1_4;JavaxSwingLibrary"/>
		<rdfs:seeAlso rdf:resource="&j2se-1_5;JavaAwtDatatransferLibrary"/>
		<rdfs:seeAlso rdf:resource="&j2se-1_5;JavaxAccessibilityLibrary"/>
		<rdfs:seeAlso rdf:resource="&j2se-1_5;JavaLangLibrary"/>
		<rdfs:seeAlso rdf:resource="&j2se-1_5;JavaxSwingTableLibrary"/>
		<rdfs:seeAlso rdf:resource="&j2se-1_5;JavaAwtImageLibrary"/>
		<rdfs:seeAlso rdf:resource="&j2se-1_5;JavaAwtPrintLibrary"/>
		<rdfs:seeAlso rdf:resource="&j2se-1_5;JavaAwtLibrary"/>
		<rdfs:seeAlso rdf:resource="&j2se-1_5;JavaxSwingColorchooserLibrary"/>
		<rdfs:seeAlso rdf:resource="&j2se-1_5;JavaIoLibrary"/>
		<rdfs:seeAlso rdf:resource="&j2se-1_5;JavaAwtEventLibrary"/>
		<rdfs:seeAlso rdf:resource="&j2se-1_5;JavaxPrintAttributeLibrary"/>
		<rdfs:seeAlso rdf:resource="&j2se-1_5;JavaUtilLibrary"/>
		<rdfs:seeAlso rdf:resource="&j2se-1_5;JavaxSwingFilechooserLibrary"/>
		<rdfs:seeAlso rdf:resource="&j2se-1_5;JavaBeansLibrary"/>
		<rdfs:seeAlso rdf:resource="&j2se-1_5;JavaxSwingEventLibrary"/>
		<rdfs:seeAlso rdf:resource="&j2se-1_5;JavaTextLibrary"/>
		<rdfs:seeAlso rdf:resource="&j2se-1_5;JavaxSwingPlafLibrary"/>
		<rdfs:seeAlso rdf:resource="&j2se-1_5;JavaxSwingBorderLibrary"/>
		<rdfs:seeAlso rdf:resource="&j2se-1_5;JavaAppletLibrary"/>
		<rdfs:seeAlso rdf:resource="&j2se-1_5;JavaxSwingTextLibrary"/>
		<rdfs:seeAlso rdf:resource="&j2se-1_5;JavaNetLibrary"/>
		<rdfs:seeAlso rdf:resource="&j2se-1_5;JavaxSwingTreeLibrary"/>
		<rdfs:comment xml:lang="en">JavaLibrary implementing the javax.swing package for j2se-1_5</rdfs:comment>
	</owl:Class>
	<owl:Class rdf:about="&j2se-1_5;JavaLangInstrumentLibrary">
		<rdfs:subClassOf rdf:resource="&java;JavaLibrary"/>
		<rdfs:seeAlso rdf:resource="&j2se-1_5;JavaSecurityLibrary"/>
		<rdfs:seeAlso rdf:resource="&j2se-1_5;JavaLangLibrary"/>
		<rdfs:comment xml:lang="en">JavaLibrary implementing the java.lang.instrument package for j2se-1_5</rdfs:comment>
	</owl:Class>
	<owl:Class rdf:about="&j2se-1_5;JavaxTransactionXaLibrary">
		<owl:equivalentClass rdf:resource="&j2se-1_4;JavaxTransactionXaLibrary"/>
		<rdfs:subClassOf rdf:resource="&java;JavaLibrary"/>
		<rdfs:seeAlso rdf:resource="&j2se-1_5;JavaLangLibrary"/>
		<rdfs:comment xml:lang="en">JavaLibrary implementing the javax.transaction.xa package for j2se-1_5</rdfs:comment>
	</owl:Class>
	<owl:Class rdf:about="&j2se-1_5;JavaAppletLibrary">
		<rdfs:subClassOf rdf:resource="&j2se-1_4;JavaAppletLibrary"/>
		<rdfs:seeAlso rdf:resource="&j2se-1_5;JavaxAccessibilityLibrary"/>
		<rdfs:seeAlso rdf:resource="&j2se-1_5;JavaIoLibrary"/>
		<rdfs:seeAlso rdf:resource="&j2se-1_5;JavaLangLibrary"/>
		<rdfs:seeAlso rdf:resource="&j2se-1_5;JavaAwtLibrary"/>
		<rdfs:seeAlso rdf:resource="&j2se-1_5;JavaNetLibrary"/>
		<rdfs:seeAlso rdf:resource="&j2se-1_5;JavaUtilLibrary"/>
		<rdfs:comment xml:lang="en">JavaLibrary implementing the java.applet package for j2se-1_5</rdfs:comment>
	</owl:Class>
	<owl:Class rdf:about="&j2se-1_5;JavaxSwingTextLibrary">
		<rdfs:subClassOf rdf:resource="&j2se-1_4;JavaxSwingTextLibrary"/>
		<rdfs:seeAlso rdf:resource="&j2se-1_5;JavaAwtImLibrary"/>
		<rdfs:seeAlso rdf:resource="&j2se-1_5;JavaUtilLibrary"/>
		<rdfs:seeAlso rdf:resource="&j2se-1_5;JavaxAccessibilityLibrary"/>
		<rdfs:seeAlso rdf:resource="&j2se-1_5;JavaLangLibrary"/>
		<rdfs:seeAlso rdf:resource="&j2se-1_5;JavaxSwingEventLibrary"/>
		<rdfs:seeAlso rdf:resource="&j2se-1_5;JavaAwtLibrary"/>
		<rdfs:seeAlso rdf:resource="&j2se-1_5;JavaTextLibrary"/>
		<rdfs:seeAlso rdf:resource="&j2se-1_5;JavaxSwingPlafLibrary"/>
		<rdfs:seeAlso rdf:resource="&j2se-1_5;JavaxSwingPlafBasicLibrary"/>
		<rdfs:seeAlso rdf:resource="&j2se-1_5;JavaxSwingLibrary"/>
		<rdfs:seeAlso rdf:resource="&j2se-1_5;JavaIoLibrary"/>
		<rdfs:seeAlso rdf:resource="&j2se-1_5;JavaAwtEventLibrary"/>
		<rdfs:seeAlso rdf:resource="&j2se-1_5;JavaxSwingUndoLibrary"/>
		<rdfs:seeAlso rdf:resource="&j2se-1_5;JavaxSwingTreeLibrary"/>
		<rdfs:comment xml:lang="en">JavaLibrary implementing the javax.swing.text package for j2se-1_5</rdfs:comment>
	</owl:Class>
	<owl:Class rdf:about="&j2se-1_5;JavaNioLibrary">
		<rdfs:subClassOf rdf:resource="&j2se-1_4;JavaNioLibrary"/>
		<rdfs:seeAlso rdf:resource="&j2se-1_5;JavaLangLibrary"/>
		<rdfs:comment xml:lang="en">JavaLibrary implementing the java.nio package for j2se-1_5</rdfs:comment>
	</owl:Class>
	<owl:Class rdf:about="&j2se-1_5;JavaxSoundMidiLibrary">
		<rdfs:subClassOf rdf:resource="&java;JavaLibrary"/>
		<rdfs:seeAlso rdf:resource="&j2se-1_5;JavaIoLibrary"/>
		<rdfs:seeAlso rdf:resource="&j2se-1_5;JavaLangLibrary"/>
		<rdfs:seeAlso rdf:resource="&j2se-1_5;JavaNetLibrary"/>
		<rdfs:seeAlso rdf:resource="&j2se-1_5;JavaUtilLibrary"/>
		<rdfs:comment xml:lang="en">JavaLibrary implementing the javax.sound.midi package for j2se-1_5</rdfs:comment>
	</owl:Class>
	<owl:Class rdf:about="&j2se-1_5;JavaUtilLoggingLibrary">
		<rdfs:subClassOf rdf:resource="&j2se-1_4;JavaUtilLoggingLibrary"/>
		<rdfs:seeAlso rdf:resource="&j2se-1_5;JavaBeansLibrary"/>
		<rdfs:seeAlso rdf:resource="&j2se-1_5;JavaIoLibrary"/>
		<rdfs:seeAlso rdf:resource="&j2se-1_5;JavaLangLibrary"/>
		<rdfs:seeAlso rdf:resource="&j2se-1_5;JavaSecurityLibrary"/>
		<rdfs:seeAlso rdf:resource="&j2se-1_5;JavaUtilLibrary"/>
		<rdfs:comment xml:lang="en">JavaLibrary implementing the java.util.logging package for j2se-1_5</rdfs:comment>
	</owl:Class>
	<owl:Class rdf:about="&j2se-1_5;OrgW3cDomEventsLibrary">
		<owl:equivalentClass rdf:resource="&j2se-1_4;OrgW3cDomEventsLibrary"/>
		<rdfs:subClassOf rdf:resource="&java;JavaLibrary"/>
		<rdfs:seeAlso rdf:resource="&j2se-1_5;OrgW3cDomViewsLibrary"/>
		<rdfs:seeAlso rdf:resource="&j2se-1_5;JavaLangLibrary"/>
		<rdfs:seeAlso rdf:resource="&j2se-1_5;OrgW3cDomLibrary"/>
		<rdfs:comment xml:lang="en">JavaLibrary implementing the org.w3c.dom.events package for j2se-1_5</rdfs:comment>
	</owl:Class>
	<owl:Class rdf:about="&j2se-1_5;JavaxSqlRowsetLibrary">
		<rdfs:subClassOf rdf:resource="&java;JavaLibrary"/>
		<rdfs:seeAlso rdf:resource="&j2se-1_5;JavaxSqlLibrary"/>
		<rdfs:seeAlso rdf:resource="&j2se-1_5;JavaSqlLibrary"/>
		<rdfs:seeAlso rdf:resource="&j2se-1_5;JavaUtilLibrary"/>
		<rdfs:seeAlso rdf:resource="&j2se-1_5;JavaIoLibrary"/>
		<rdfs:seeAlso rdf:resource="&j2se-1_5;JavaLangLibrary"/>
		<rdfs:seeAlso rdf:resource="&j2se-1_5;JavaxSqlRowsetSpiLibrary"/>
		<rdfs:seeAlso rdf:resource="&j2se-1_5;JavaMathLibrary"/>
		<rdfs:comment xml:lang="en">JavaLibrary implementing the javax.sql.rowset package for j2se-1_5</rdfs:comment>
	</owl:Class>
	<owl:Class rdf:about="&j2se-1_5;JavaRmiDgcLibrary">
		<owl:equivalentClass rdf:resource="&j2se-1_4;JavaRmiDgcLibrary"/>
		<rdfs:subClassOf rdf:resource="&java;JavaLibrary"/>
		<rdfs:seeAlso rdf:resource="&j2se-1_5;JavaRmiLibrary"/>
		<rdfs:seeAlso rdf:resource="&j2se-1_5;JavaIoLibrary"/>
		<rdfs:seeAlso rdf:resource="&j2se-1_5;JavaLangLibrary"/>
		<rdfs:comment xml:lang="en">JavaLibrary implementing the java.rmi.dgc package for j2se-1_5</rdfs:comment>
	</owl:Class>
	<owl:Class rdf:about="&j2se-1_5;JavaxSqlRowsetSpiLibrary">
		<rdfs:subClassOf rdf:resource="&java;JavaLibrary"/>
		<rdfs:seeAlso rdf:resource="&j2se-1_5;JavaxSqlLibrary"/>
		<rdfs:seeAlso rdf:resource="&j2se-1_5;JavaIoLibrary"/>
		<rdfs:seeAlso rdf:resource="&j2se-1_5;JavaSqlLibrary"/>
		<rdfs:seeAlso rdf:resource="&j2se-1_5;JavaLangLibrary"/>
		<rdfs:seeAlso rdf:resource="&j2se-1_5;JavaUtilLoggingLibrary"/>
		<rdfs:seeAlso rdf:resource="&j2se-1_5;JavaxSqlRowsetLibrary"/>
		<rdfs:seeAlso rdf:resource="&j2se-1_5;JavaxNamingLibrary"/>
		<rdfs:seeAlso rdf:resource="&j2se-1_5;JavaUtilLibrary"/>
		<rdfs:comment xml:lang="en">JavaLibrary implementing the javax.sql.rowset.spi package for j2se-1_5</rdfs:comment>
	</owl:Class>
	<owl:Class rdf:about="&j2se-1_5;JavaSecurityInterfacesLibrary">
		<rdfs:subClassOf rdf:resource="&j2se-1_4;JavaSecurityInterfacesLibrary"/>
		<rdfs:seeAlso rdf:resource="&j2se-1_5;JavaSecuritySpecLibrary"/>
		<rdfs:seeAlso rdf:resource="&j2se-1_5;JavaSecurityLibrary"/>
		<rdfs:seeAlso rdf:resource="&j2se-1_5;JavaMathLibrary"/>
		<rdfs:comment xml:lang="en">JavaLibrary implementing the java.security.interfaces package for j2se-1_5</rdfs:comment>
	</owl:Class>
	<owl:Class rdf:about="&j2se-1_5;JavaxManagementMonitorLibrary">
		<rdfs:subClassOf rdf:resource="&java;JavaLibrary"/>
		<rdfs:seeAlso rdf:resource="&j2se-1_5;JavaxManagementLibrary"/>
		<rdfs:seeAlso rdf:resource="&j2se-1_5;JavaLangLibrary"/>
		<rdfs:comment xml:lang="en">JavaLibrary implementing the javax.management.monitor package for j2se-1_5</rdfs:comment>
	</owl:Class>
	<owl:Class rdf:about="&j2se-1_5;OrgOmgPortableServerServantLocatorPackageLibrary">
		<owl:equivalentClass rdf:resource="&j2se-1_4;OrgOmgPortableServerServantLocatorPackageLibrary"/>
		<rdfs:subClassOf rdf:resource="&java;JavaLibrary"/>
		<rdfs:seeAlso rdf:resource="&j2se-1_5;OrgOmgCORBAPortableLibrary"/>
		<rdfs:seeAlso rdf:resource="&j2se-1_5;OrgOmgCORBALibrary"/>
		<rdfs:seeAlso rdf:resource="&j2se-1_5;JavaLangLibrary"/>
		<rdfs:comment xml:lang="en">JavaLibrary implementing the org.omg.PortableServer.ServantLocatorPackage package for j2se-1_5</rdfs:comment>
	</owl:Class>
	<owl:Class rdf:about="&j2se-1_5;JavaxXmlParsersLibrary">
		<rdfs:subClassOf rdf:resource="&j2se-1_4;JavaxXmlParsersLibrary"/>
		<rdfs:seeAlso rdf:resource="&j2se-1_5;JavaIoLibrary"/>
		<rdfs:seeAlso rdf:resource="&j2se-1_5;JavaLangLibrary"/>
		<rdfs:seeAlso rdf:resource="&j2se-1_5;OrgXmlSaxLibrary"/>
		<rdfs:seeAlso rdf:resource="&j2se-1_5;OrgXmlSaxHelpersLibrary"/>
		<rdfs:seeAlso rdf:resource="&j2se-1_5;JavaxXmlValidationLibrary"/>
		<rdfs:seeAlso rdf:resource="&j2se-1_5;OrgW3cDomLibrary"/>
		<rdfs:comment xml:lang="en">JavaLibrary implementing the javax.xml.parsers package for j2se-1_5</rdfs:comment>
	</owl:Class>
	<owl:Class rdf:about="&j2se-1_5;JavaNetLibrary">
		<rdfs:subClassOf rdf:resource="&j2se-1_4;JavaNetLibrary"/>
		<rdfs:seeAlso rdf:resource="&j2se-1_5;JavaUtilJarLibrary"/>
		<rdfs:seeAlso rdf:resource="&j2se-1_5;JavaSecurityLibrary"/>
		<rdfs:seeAlso rdf:resource="&j2se-1_5;JavaUtilLibrary"/>
		<rdfs:seeAlso rdf:resource="&j2se-1_5;JavaIoLibrary"/>
		<rdfs:seeAlso rdf:resource="&j2se-1_5;JavaLangLibrary"/>
		<rdfs:seeAlso rdf:resource="&j2se-1_5;JavaNioChannelsLibrary"/>
		<rdfs:comment xml:lang="en">JavaLibrary implementing the java.net package for j2se-1_5</rdfs:comment>
	</owl:Class>
	<owl:Class rdf:about="&j2se-1_5;OrgOmgPortableServerLibrary">
		<rdfs:subClassOf rdf:resource="&j2se-1_4;OrgOmgPortableServerLibrary"/>
		<rdfs:seeAlso rdf:resource="&j2se-1_5;OrgOmgCORBAPortableLibrary"/>
		<rdfs:seeAlso rdf:resource="&j2se-1_5;JavaLangLibrary"/>
		<rdfs:seeAlso rdf:resource="&j2se-1_5;OrgOmgPortableServerPortableLibrary"/>
		<rdfs:seeAlso rdf:resource="&j2se-1_5;OrgOmgPortableServerServantLocatorPackageLibrary"/>
		<rdfs:seeAlso rdf:resource="&j2se-1_5;OrgOmgCORBALibrary"/>
		<rdfs:seeAlso rdf:resource="&j2se-1_5;OrgOmgPortableServerPOAManagerPackageLibrary"/>
		<rdfs:comment xml:lang="en">JavaLibrary implementing the org.omg.PortableServer package for j2se-1_5</rdfs:comment>
	</owl:Class>
	<owl:Class rdf:about="&j2se-1_5;OrgW3cDomCssLibrary">
		<rdfs:subClassOf rdf:resource="&j2se-1_4;OrgW3cDomCssLibrary"/>
		<rdfs:seeAlso rdf:resource="&j2se-1_5;OrgW3cDomViewsLibrary"/>
		<rdfs:seeAlso rdf:resource="&j2se-1_5;JavaLangLibrary"/>
		<rdfs:seeAlso rdf:resource="&j2se-1_5;OrgW3cDomStylesheetsLibrary"/>
		<rdfs:seeAlso rdf:resource="&j2se-1_5;OrgW3cDomLibrary"/>
		<rdfs:comment xml:lang="en">JavaLibrary implementing the org.w3c.dom.css package for j2se-1_5</rdfs:comment>
	</owl:Class>
	<owl:Class rdf:about="&j2se-1_5;JavaxSwingUndoLibrary">
		<owl:equivalentClass rdf:resource="&j2se-1_4;JavaxSwingUndoLibrary"/>
		<rdfs:subClassOf rdf:resource="&java;JavaLibrary"/>
		<rdfs:seeAlso rdf:resource="&j2se-1_5;JavaIoLibrary"/>
		<rdfs:seeAlso rdf:resource="&j2se-1_5;JavaLangLibrary"/>
		<rdfs:seeAlso rdf:resource="&j2se-1_5;JavaUtilLibrary"/>
		<rdfs:seeAlso rdf:resource="&j2se-1_5;JavaxSwingEventLibrary"/>
		<rdfs:comment xml:lang="en">JavaLibrary implementing the javax.swing.undo package for j2se-1_5</rdfs:comment>
	</owl:Class>
	<owl:Class rdf:about="&j2se-1_5;JavaxSoundSampledSpiLibrary">
		<owl:equivalentClass rdf:resource="&j2se-1_4;JavaxSoundSampledSpiLibrary"/>
		<rdfs:subClassOf rdf:resource="&java;JavaLibrary"/>
		<rdfs:seeAlso rdf:resource="&j2se-1_5;JavaIoLibrary"/>
		<rdfs:seeAlso rdf:resource="&j2se-1_5;JavaLangLibrary"/>
		<rdfs:seeAlso rdf:resource="&j2se-1_5;JavaNetLibrary"/>
		<rdfs:seeAlso rdf:resource="&j2se-1_5;JavaxSoundSampledLibrary"/>
		<rdfs:comment xml:lang="en">JavaLibrary implementing the javax.sound.sampled.spi package for j2se-1_5</rdfs:comment>
	</owl:Class>
	<owl:Class rdf:about="&j2se-1_5;JavaxSecurityAuthSpiLibrary">
		<owl:equivalentClass rdf:resource="&j2se-1_4;JavaxSecurityAuthSpiLibrary"/>
		<rdfs:subClassOf rdf:resource="&java;JavaLibrary"/>
		<rdfs:seeAlso rdf:resource="&j2se-1_5;JavaxSecurityAuthLibrary"/>
		<rdfs:seeAlso rdf:resource="&j2se-1_5;JavaUtilLibrary"/>
		<rdfs:seeAlso rdf:resource="&j2se-1_5;JavaxSecurityAuthCallbackLibrary"/>
		<rdfs:comment xml:lang="en">JavaLibrary implementing the javax.security.auth.spi package for j2se-1_5</rdfs:comment>
	</owl:Class>
	<owl:Class rdf:about="&j2se-1_5;OrgOmgDynamicAnyDynAnyPackageLibrary">
		<owl:equivalentClass rdf:resource="&j2se-1_4;OrgOmgDynamicAnyDynAnyPackageLibrary"/>
		<rdfs:subClassOf rdf:resource="&java;JavaLibrary"/>
		<rdfs:seeAlso rdf:resource="&j2se-1_5;OrgOmgCORBAPortableLibrary"/>
		<rdfs:seeAlso rdf:resource="&j2se-1_5;OrgOmgCORBALibrary"/>
		<rdfs:seeAlso rdf:resource="&j2se-1_5;JavaLangLibrary"/>
		<rdfs:comment xml:lang="en">JavaLibrary implementing the org.omg.DynamicAny.DynAnyPackage package for j2se-1_5</rdfs:comment>
	</owl:Class>
	<owl:Class rdf:about="&j2se-1_5;OrgOmgPortableServerCurrentPackageLibrary">
		<owl:equivalentClass rdf:resource="&j2se-1_4;OrgOmgPortableServerCurrentPackageLibrary"/>
		<rdfs:subClassOf rdf:resource="&java;JavaLibrary"/>
		<rdfs:seeAlso rdf:resource="&j2se-1_5;OrgOmgCORBAPortableLibrary"/>
		<rdfs:seeAlso rdf:resource="&j2se-1_5;OrgOmgCORBALibrary"/>
		<rdfs:seeAlso rdf:resource="&j2se-1_5;JavaLangLibrary"/>
		<rdfs:comment xml:lang="en">JavaLibrary implementing the org.omg.PortableServer.CurrentPackage package for j2se-1_5</rdfs:comment>
	</owl:Class>
	<owl:Class rdf:about="&j2se-1_5;OrgOmgCosNamingNamingContextExtPackageLibrary">
		<owl:equivalentClass rdf:resource="&j2se-1_4;OrgOmgCosNamingNamingContextExtPackageLibrary"/>
		<rdfs:subClassOf rdf:resource="&java;JavaLibrary"/>
		<rdfs:seeAlso rdf:resource="&j2se-1_5;OrgOmgCORBAPortableLibrary"/>
		<rdfs:seeAlso rdf:resource="&j2se-1_5;OrgOmgCORBALibrary"/>
		<rdfs:seeAlso rdf:resource="&j2se-1_5;JavaLangLibrary"/>
		<rdfs:comment xml:lang="en">JavaLibrary implementing the org.omg.CosNaming.NamingContextExtPackage package for j2se-1_5</rdfs:comment>
	</owl:Class>
	<owl:Class rdf:about="&j2se-1_5;JavaAwtColorLibrary">
		<rdfs:subClassOf rdf:resource="&j2se-1_4;JavaAwtColorLibrary"/>
		<rdfs:seeAlso rdf:resource="&j2se-1_5;JavaIoLibrary"/>
		<rdfs:seeAlso rdf:resource="&j2se-1_5;JavaLangLibrary"/>
		<rdfs:comment xml:lang="en">JavaLibrary implementing the java.awt.color package for j2se-1_5</rdfs:comment>
	</owl:Class>
	<owl:Class rdf:about="&j2se-1_5;OrgOmgCORBAORBPackageLibrary">
		<owl:equivalentClass rdf:resource="&j2se-1_4;OrgOmgCORBAORBPackageLibrary"/>
		<rdfs:subClassOf rdf:resource="&java;JavaLibrary"/>
		<rdfs:seeAlso rdf:resource="&j2se-1_5;OrgOmgCORBALibrary"/>
		<rdfs:seeAlso rdf:resource="&j2se-1_5;JavaLangLibrary"/>
		<rdfs:comment xml:lang="en">JavaLibrary implementing the org.omg.CORBA.ORBPackage package for j2se-1_5</rdfs:comment>
	</owl:Class>
	<owl:Class rdf:about="&j2se-1_5;JavaxSwingTreeLibrary">
		<rdfs:subClassOf rdf:resource="&j2se-1_4;JavaxSwingTreeLibrary"/>
		<rdfs:seeAlso rdf:resource="&j2se-1_5;JavaUtilLibrary"/>
		<rdfs:seeAlso rdf:resource="&j2se-1_5;JavaxSwingBorderLibrary"/>
		<rdfs:seeAlso rdf:resource="&j2se-1_5;JavaxSwingLibrary"/>
		<rdfs:seeAlso rdf:resource="&j2se-1_5;JavaBeansLibrary"/>
		<rdfs:seeAlso rdf:resource="&j2se-1_5;JavaIoLibrary"/>
		<rdfs:seeAlso rdf:resource="&j2se-1_5;JavaAwtEventLibrary"/>
		<rdfs:seeAlso rdf:resource="&j2se-1_5;JavaLangLibrary"/>
		<rdfs:seeAlso rdf:resource="&j2se-1_5;JavaxSwingEventLibrary"/>
		<rdfs:seeAlso rdf:resource="&j2se-1_5;JavaAwtLibrary"/>
		<rdfs:comment xml:lang="en">JavaLibrary implementing the javax.swing.tree package for j2se-1_5</rdfs:comment>
	</owl:Class>
	<owl:Class rdf:about="&j2se-1_5;JavaxSoundSampledLibrary">
		<rdfs:subClassOf rdf:resource="&j2se-1_4;JavaxSoundSampledLibrary"/>
		<rdfs:seeAlso rdf:resource="&j2se-1_5;JavaIoLibrary"/>
		<rdfs:seeAlso rdf:resource="&j2se-1_5;JavaLangLibrary"/>
		<rdfs:seeAlso rdf:resource="&j2se-1_5;JavaNetLibrary"/>
		<rdfs:seeAlso rdf:resource="&j2se-1_5;JavaSecurityLibrary"/>
		<rdfs:seeAlso rdf:resource="&j2se-1_5;JavaUtilLibrary"/>
		<rdfs:comment xml:lang="en">JavaLibrary implementing the javax.sound.sampled package for j2se-1_5</rdfs:comment>
	</owl:Class>
	<owl:Class rdf:about="&j2se-1_5;JavaUtilConcurrentLibrary">
		<rdfs:subClassOf rdf:resource="&java;JavaLibrary"/>
		<rdfs:seeAlso rdf:resource="&j2se-1_5;JavaSecurityLibrary"/>
		<rdfs:seeAlso rdf:resource="&j2se-1_5;JavaUtilLibrary"/>
		<rdfs:seeAlso rdf:resource="&j2se-1_5;JavaIoLibrary"/>
		<rdfs:seeAlso rdf:resource="&j2se-1_5;JavaLangLibrary"/>
		<rdfs:comment xml:lang="en">JavaLibrary implementing the java.util.concurrent package for j2se-1_5</rdfs:comment>
	</owl:Class>
</rdf:RDF>
