<?xml version="1.0" encoding="ISO-8859-1"?>
<!DOCTYPE rdf:RDF [
	<!ENTITY xsd "http://www.w3.org/2001/XMLSchema#">
	<!ENTITY platform "http://localhost/~dennis/Platform.owl#">
	<!ENTITY swt-3_4 "http://ssel.vub.ac.be/platformkit/swt-3_4#">
	<!ENTITY java "http://localhost/~dennis/Java.owl#">
	<!ENTITY swt-3_3 "http://ssel.vub.ac.be/platformkit/swt-3_3#">
	<!ENTITY units "http://localhost/~dennis/Units.owl#">
	<!ENTITY rdf "http://www.w3.org/1999/02/22-rdf-syntax-ns#">
	<!ENTITY rdfs "http://www.w3.org/2000/01/rdf-schema#">
	<!ENTITY owl "http://www.w3.org/2002/07/owl#">
]>
<rdf:RDF
	 xmlns:xsd="&xsd;"
	 xmlns:platform="&platform;"
	 xmlns:swt-3_4="&swt-3_4;"
	 xmlns:java="&java;"
	 xmlns:swt-3_3="&swt-3_3;"
	 xmlns:units="&units;"
	 xmlns:rdf="&rdf;"
	 xmlns:rdfs="&rdfs;"
	 xmlns:owl="&owl;"
>

	<owl:Ontology rdf:about="http://ssel.vub.ac.be/platformkit/swt-3_4#">
		<owl:imports rdf:resource="http://localhost/~dennis/Platform.owl"/>
		<owl:imports rdf:resource="http://localhost/~dennis/Java.owl"/>
		<owl:imports rdf:resource="http://ssel.vub.ac.be/platformkit/swt-3_3#"/>
		<rdfs:comment xml:lang="en">Generated by $Id: UML2ToPackageAPIOntology.atl 7380 2007-11-08 09:49:02Z dwagelaa $ and $Id: UML2ToAPIOntology.atl 7380 2007-11-08 09:49:02Z dwagelaa $ and $Id:UML2Comparison.atl 7084 2007-07-10 13:19:05Z dwagelaa $</rdfs:comment>
		<rdfs:label xml:lang="en">swt-3_4</rdfs:label>
	</owl:Ontology>
	<owl:Class rdf:about="&swt-3_4;Swt-3_4ClassLibrary">
		<rdfs:subClassOf rdf:resource="&swt-3_4;OrgEclipseSwtLibrary"/>
		<rdfs:subClassOf rdf:resource="&swt-3_4;OrgEclipseSwtAccessibilityLibrary"/>
		<rdfs:subClassOf rdf:resource="&swt-3_4;OrgEclipseSwtAwtLibrary"/>
		<rdfs:subClassOf rdf:resource="&swt-3_4;OrgEclipseSwtBrowserLibrary"/>
		<rdfs:subClassOf rdf:resource="&swt-3_4;OrgEclipseSwtWidgetsLibrary"/>
		<rdfs:subClassOf rdf:resource="&swt-3_4;OrgEclipseSwtEventsLibrary"/>
		<rdfs:subClassOf rdf:resource="&swt-3_4;OrgEclipseSwtCustomLibrary"/>
		<rdfs:subClassOf rdf:resource="&swt-3_4;OrgEclipseSwtGraphicsLibrary"/>
		<rdfs:subClassOf rdf:resource="&swt-3_4;OrgEclipseSwtDndLibrary"/>
		<rdfs:subClassOf rdf:resource="&swt-3_4;OrgEclipseSwtLayoutLibrary"/>
		<rdfs:subClassOf rdf:resource="&swt-3_4;OrgEclipseSwtOpenglLibrary"/>
		<rdfs:subClassOf rdf:resource="&swt-3_4;OrgEclipseSwtPrintingLibrary"/>
		<rdfs:subClassOf rdf:resource="&swt-3_4;OrgEclipseSwtProgramLibrary"/>
		<rdfs:subClassOf rdf:resource="&swt-3_4;JavaLangLibrary"/>
		<rdfs:subClassOf rdf:resource="&swt-3_4;JavaUtilLibrary"/>
		<rdfs:subClassOf rdf:resource="&swt-3_4;JavaIoLibrary"/>
		<rdfs:comment xml:lang="en">JavaLibrary implementing the entire API for swt-3_4</rdfs:comment>
	</owl:Class>
	<owl:Class rdf:about="&swt-3_4;Swt-3_4">
		<rdfs:subClassOf rdf:resource="&java;JRE"/>
		<rdfs:subClassOf>
			<owl:Restriction>
				<owl:onProperty rdf:resource="&java;providesBuiltinJavaLibrary"/>
				<owl:someValuesFrom rdf:resource="&swt-3_4;Swt-3_4ClassLibrary"/>
			</owl:Restriction>
		</rdfs:subClassOf>
		<rdfs:comment xml:lang="en">swt-3_4 Java Runtime Environment</rdfs:comment>
	</owl:Class>
	<owl:Class rdf:about="&swt-3_4;OrgEclipseSwtLibrary">
		<rdfs:subClassOf rdf:resource="&swt-3_3;OrgEclipseSwtLibrary"/>
		<rdfs:seeAlso rdf:resource="&swt-3_4;JavaLangLibrary"/>
		<rdfs:comment xml:lang="en">JavaLibrary implementing the org.eclipse.swt package for swt-3_4</rdfs:comment>
	</owl:Class>
	<owl:Class rdf:about="&swt-3_4;OrgEclipseSwtAccessibilityLibrary">
		<owl:equivalentClass rdf:resource="&swt-3_3;OrgEclipseSwtAccessibilityLibrary"/>
		<rdfs:subClassOf rdf:resource="&java;JavaLibrary"/>
		<rdfs:seeAlso rdf:resource="&swt-3_4;JavaLangLibrary"/>
		<rdfs:seeAlso rdf:resource="&swt-3_4;OrgEclipseSwtWidgetsLibrary"/>
		<rdfs:comment xml:lang="en">JavaLibrary implementing the org.eclipse.swt.accessibility package for swt-3_4</rdfs:comment>
	</owl:Class>
	<owl:Class rdf:about="&swt-3_4;OrgEclipseSwtAwtLibrary">
		<owl:equivalentClass rdf:resource="&swt-3_3;OrgEclipseSwtAwtLibrary"/>
		<rdfs:subClassOf rdf:resource="&java;JavaLibrary"/>
		<rdfs:seeAlso rdf:resource="&swt-3_4;JavaLangLibrary"/>
		<rdfs:seeAlso rdf:resource="&swt-3_4;OrgEclipseSwtWidgetsLibrary"/>
		<rdfs:comment xml:lang="en">JavaLibrary implementing the org.eclipse.swt.awt package for swt-3_4</rdfs:comment>
	</owl:Class>
	<owl:Class rdf:about="&swt-3_4;OrgEclipseSwtBrowserLibrary">
		<rdfs:subClassOf rdf:resource="&swt-3_3;OrgEclipseSwtBrowserLibrary"/>
		<rdfs:seeAlso rdf:resource="&swt-3_4;OrgEclipseSwtGraphicsLibrary"/>
		<rdfs:seeAlso rdf:resource="&swt-3_4;OrgEclipseSwtEventsLibrary"/>
		<rdfs:seeAlso rdf:resource="&swt-3_4;JavaLangLibrary"/>
		<rdfs:seeAlso rdf:resource="&swt-3_4;OrgEclipseSwtWidgetsLibrary"/>
		<rdfs:comment xml:lang="en">JavaLibrary implementing the org.eclipse.swt.browser package for swt-3_4</rdfs:comment>
	</owl:Class>
	<owl:Class rdf:about="&swt-3_4;OrgEclipseSwtWidgetsLibrary">
		<rdfs:subClassOf rdf:resource="&swt-3_3;OrgEclipseSwtWidgetsLibrary"/>
		<rdfs:seeAlso rdf:resource="&swt-3_4;OrgEclipseSwtGraphicsLibrary"/>
		<rdfs:seeAlso rdf:resource="&swt-3_4;OrgEclipseSwtAccessibilityLibrary"/>
		<rdfs:seeAlso rdf:resource="&swt-3_4;OrgEclipseSwtEventsLibrary"/>
		<rdfs:seeAlso rdf:resource="&swt-3_4;JavaLangLibrary"/>
		<rdfs:comment xml:lang="en">JavaLibrary implementing the org.eclipse.swt.widgets package for swt-3_4</rdfs:comment>
	</owl:Class>
	<owl:Class rdf:about="&swt-3_4;OrgEclipseSwtEventsLibrary">
		<owl:equivalentClass rdf:resource="&swt-3_3;OrgEclipseSwtEventsLibrary"/>
		<rdfs:subClassOf rdf:resource="&java;JavaLibrary"/>
		<rdfs:seeAlso rdf:resource="&swt-3_4;OrgEclipseSwtGraphicsLibrary"/>
		<rdfs:seeAlso rdf:resource="&swt-3_4;JavaLangLibrary"/>
		<rdfs:seeAlso rdf:resource="&swt-3_4;OrgEclipseSwtWidgetsLibrary"/>
		<rdfs:comment xml:lang="en">JavaLibrary implementing the org.eclipse.swt.events package for swt-3_4</rdfs:comment>
	</owl:Class>
	<owl:Class rdf:about="&swt-3_4;OrgEclipseSwtCustomLibrary">
		<rdfs:subClassOf rdf:resource="&swt-3_3;OrgEclipseSwtCustomLibrary"/>
		<rdfs:seeAlso rdf:resource="&swt-3_4;OrgEclipseSwtGraphicsLibrary"/>
		<rdfs:seeAlso rdf:resource="&swt-3_4;OrgEclipseSwtWidgetsLibrary"/>
		<rdfs:seeAlso rdf:resource="&swt-3_4;OrgEclipseSwtDndLibrary"/>
		<rdfs:seeAlso rdf:resource="&swt-3_4;OrgEclipseSwtEventsLibrary"/>
		<rdfs:seeAlso rdf:resource="&swt-3_4;JavaLangLibrary"/>
		<rdfs:seeAlso rdf:resource="&swt-3_4;OrgEclipseSwtPrintingLibrary"/>
		<rdfs:comment xml:lang="en">JavaLibrary implementing the org.eclipse.swt.custom package for swt-3_4</rdfs:comment>
	</owl:Class>
	<owl:Class rdf:about="&swt-3_4;OrgEclipseSwtGraphicsLibrary">
		<rdfs:subClassOf rdf:resource="&swt-3_3;OrgEclipseSwtGraphicsLibrary"/>
		<rdfs:seeAlso rdf:resource="&swt-3_4;JavaLangLibrary"/>
		<rdfs:seeAlso rdf:resource="&swt-3_4;JavaIoLibrary"/>
		<rdfs:comment xml:lang="en">JavaLibrary implementing the org.eclipse.swt.graphics package for swt-3_4</rdfs:comment>
	</owl:Class>
	<owl:Class rdf:about="&swt-3_4;OrgEclipseSwtDndLibrary">
		<rdfs:subClassOf rdf:resource="&swt-3_3;OrgEclipseSwtDndLibrary"/>
		<rdfs:seeAlso rdf:resource="&swt-3_4;OrgEclipseSwtGraphicsLibrary"/>
		<rdfs:seeAlso rdf:resource="&swt-3_4;OrgEclipseSwtEventsLibrary"/>
		<rdfs:seeAlso rdf:resource="&swt-3_4;JavaLangLibrary"/>
		<rdfs:seeAlso rdf:resource="&swt-3_4;OrgEclipseSwtWidgetsLibrary"/>
		<rdfs:comment xml:lang="en">JavaLibrary implementing the org.eclipse.swt.dnd package for swt-3_4</rdfs:comment>
	</owl:Class>
	<owl:Class rdf:about="&swt-3_4;OrgEclipseSwtLayoutLibrary">
		<rdfs:subClassOf rdf:resource="&swt-3_3;OrgEclipseSwtLayoutLibrary"/>
		<rdfs:seeAlso rdf:resource="&swt-3_4;OrgEclipseSwtGraphicsLibrary"/>
		<rdfs:seeAlso rdf:resource="&swt-3_4;JavaLangLibrary"/>
		<rdfs:seeAlso rdf:resource="&swt-3_4;OrgEclipseSwtWidgetsLibrary"/>
		<rdfs:comment xml:lang="en">JavaLibrary implementing the org.eclipse.swt.layout package for swt-3_4</rdfs:comment>
	</owl:Class>
	<owl:Class rdf:about="&swt-3_4;OrgEclipseSwtOpenglLibrary">
		<rdfs:subClassOf rdf:resource="&swt-3_3;OrgEclipseSwtOpenglLibrary"/>
		<rdfs:seeAlso rdf:resource="&swt-3_4;JavaLangLibrary"/>
		<rdfs:seeAlso rdf:resource="&swt-3_4;OrgEclipseSwtWidgetsLibrary"/>
		<rdfs:comment xml:lang="en">JavaLibrary implementing the org.eclipse.swt.opengl package for swt-3_4</rdfs:comment>
	</owl:Class>
	<owl:Class rdf:about="&swt-3_4;OrgEclipseSwtPrintingLibrary">
		<rdfs:subClassOf rdf:resource="&swt-3_3;OrgEclipseSwtPrintingLibrary"/>
		<rdfs:seeAlso rdf:resource="&swt-3_4;OrgEclipseSwtGraphicsLibrary"/>
		<rdfs:seeAlso rdf:resource="&swt-3_4;OrgEclipseSwtWidgetsLibrary"/>
		<rdfs:comment xml:lang="en">JavaLibrary implementing the org.eclipse.swt.printing package for swt-3_4</rdfs:comment>
	</owl:Class>
	<owl:Class rdf:about="&swt-3_4;OrgEclipseSwtProgramLibrary">
		<owl:equivalentClass rdf:resource="&swt-3_3;OrgEclipseSwtProgramLibrary"/>
		<rdfs:subClassOf rdf:resource="&java;JavaLibrary"/>
		<rdfs:seeAlso rdf:resource="&swt-3_4;OrgEclipseSwtGraphicsLibrary"/>
		<rdfs:seeAlso rdf:resource="&swt-3_4;JavaLangLibrary"/>
		<rdfs:comment xml:lang="en">JavaLibrary implementing the org.eclipse.swt.program package for swt-3_4</rdfs:comment>
	</owl:Class>
	<owl:Class rdf:about="&swt-3_4;JavaLangLibrary">
		<owl:equivalentClass rdf:resource="&swt-3_3;JavaLangLibrary"/>
		<rdfs:subClassOf rdf:resource="&java;JavaLibrary"/>
		<rdfs:comment xml:lang="en">JavaLibrary implementing the java.lang package for swt-3_4</rdfs:comment>
	</owl:Class>
	<owl:Class rdf:about="&swt-3_4;JavaUtilLibrary">
		<owl:equivalentClass rdf:resource="&swt-3_3;JavaUtilLibrary"/>
		<rdfs:subClassOf rdf:resource="&java;JavaLibrary"/>
		<rdfs:comment xml:lang="en">JavaLibrary implementing the java.util package for swt-3_4</rdfs:comment>
	</owl:Class>
	<owl:Class rdf:about="&swt-3_4;JavaIoLibrary">
		<owl:equivalentClass rdf:resource="&swt-3_3;JavaIoLibrary"/>
		<rdfs:subClassOf rdf:resource="&java;JavaLibrary"/>
		<rdfs:comment xml:lang="en">JavaLibrary implementing the java.io package for swt-3_4</rdfs:comment>
	</owl:Class>
</rdf:RDF>
