<?xml version="1.0" encoding="ISO-8859-1"?>
<!DOCTYPE rdf:RDF [
	<!ENTITY personaljava-1_1 "http://ssel.vub.ac.be/platformkit/personaljava-1_1#">
	<!ENTITY platform "http://localhost/~dennis/Platform.owl#">
	<!ENTITY xsd "http://www.w3.org/2001/XMLSchema#">
	<!ENTITY java "http://localhost/~dennis/Java.owl#">
	<!ENTITY j2me-midp-1_0 "http://ssel.vub.ac.be/platformkit/j2me-midp-1_0#">
	<!ENTITY units "http://localhost/~dennis/Units.owl#">
	<!ENTITY rdfs "http://www.w3.org/2000/01/rdf-schema#">
	<!ENTITY rdf "http://www.w3.org/1999/02/22-rdf-syntax-ns#">
	<!ENTITY ns_7 "http://localhost/~dennis/">
	<!ENTITY owl "http://www.w3.org/2002/07/owl#">
]>
<rdf:RDF
	 xmlns:personaljava-1_1="&personaljava-1_1;"
	 xmlns:platform="&platform;"
	 xmlns:xsd="&xsd;"
	 xmlns:java="&java;"
	 xmlns:j2me-midp-1_0="&j2me-midp-1_0;"
	 xmlns:units="&units;"
	 xmlns:rdfs="&rdfs;"
	 xmlns:rdf="&rdf;"
	 xmlns:ns_7="&ns_7;"
	 xmlns:owl="&owl;"
>

	<owl:Ontology rdf:about="http://ssel.vub.ac.be/platformkit/personaljava-1_1#">
		<owl:imports rdf:resource="http://localhost/~dennis/Platform.owl"/>
		<owl:imports rdf:resource="http://localhost/~dennis/Java.owl"/>
		<owl:imports rdf:resource="http://ssel.vub.ac.be/platformkit/j2me-midp-1_0#"/>
		<rdfs:comment xml:lang="en">Generated by $Id: UML2ToPackageAPIOntology.atl 6744 2007-05-25 09:44:28Z dwagelaa $</rdfs:comment>
		<rdfs:label xml:lang="en">personaljava-1_1</rdfs:label>
	</owl:Ontology>
	<owl:Class rdf:about="&personaljava-1_1;Personaljava-1_1ClassLibrary">
		<rdfs:subClassOf rdf:resource="&personaljava-1_1;JavaLangLibrary"/>
		<rdfs:subClassOf rdf:resource="&personaljava-1_1;JavaLangReflectLibrary"/>
		<rdfs:subClassOf rdf:resource="&personaljava-1_1;JavaIoLibrary"/>
		<rdfs:subClassOf rdf:resource="&personaljava-1_1;JavaUtilLibrary"/>
		<rdfs:subClassOf rdf:resource="&personaljava-1_1;JavaUtilZipLibrary"/>
		<rdfs:subClassOf rdf:resource="&personaljava-1_1;JavaTextLibrary"/>
		<rdfs:subClassOf rdf:resource="&personaljava-1_1;JavaTextResourcesLibrary"/>
		<rdfs:subClassOf rdf:resource="&personaljava-1_1;JavaNetLibrary"/>
		<rdfs:subClassOf rdf:resource="&personaljava-1_1;JavaAwtLibrary"/>
		<rdfs:subClassOf rdf:resource="&personaljava-1_1;JavaAwtImageLibrary"/>
		<rdfs:subClassOf rdf:resource="&personaljava-1_1;JavaAwtEventLibrary"/>
		<rdfs:subClassOf rdf:resource="&personaljava-1_1;JavaAwtPeerLibrary"/>
		<rdfs:subClassOf rdf:resource="&personaljava-1_1;JavaAwtDatatransferLibrary"/>
		<rdfs:subClassOf rdf:resource="&personaljava-1_1;JavaAppletLibrary"/>
		<rdfs:subClassOf rdf:resource="&personaljava-1_1;JavaBeansLibrary"/>
		<rdfs:comment xml:lang="en">JavaLibrary implementing the entire API for personaljava-1_1</rdfs:comment>
	</owl:Class>
	<owl:Class rdf:about="&personaljava-1_1;Personaljava-1_1">
		<rdfs:subClassOf rdf:resource="&java;JRE"/>
		<rdfs:subClassOf>
			<owl:Restriction>
				<owl:onProperty rdf:resource="&java;providesBuiltinJavaLibrary"/>
				<owl:someValuesFrom rdf:resource="&personaljava-1_1;Personaljava-1_1ClassLibrary"/>
			</owl:Restriction>
		</rdfs:subClassOf>
		<rdfs:comment xml:lang="en">personaljava-1_1 Java Runtime Environment</rdfs:comment>
	</owl:Class>
	<owl:Class rdf:about="&personaljava-1_1;JavaLangLibrary">
		<rdfs:subClassOf rdf:resource="&java;JavaLibrary"/>
		<rdfs:seeAlso rdf:resource="&personaljava-1_1;JavaLangReflectLibrary"/>
		<rdfs:seeAlso rdf:resource="&personaljava-1_1;JavaUtilLibrary"/>
		<rdfs:seeAlso rdf:resource="&personaljava-1_1;JavaNetLibrary"/>
		<rdfs:seeAlso rdf:resource="&personaljava-1_1;JavaIoLibrary"/>
		<rdfs:comment xml:lang="en">JavaLibrary implementing the java.lang package for personaljava-1_1</rdfs:comment>
	</owl:Class>
	<owl:Class rdf:about="&personaljava-1_1;JavaLangReflectLibrary">
		<rdfs:subClassOf rdf:resource="&java;JavaLibrary"/>
		<rdfs:seeAlso rdf:resource="&personaljava-1_1;JavaLangLibrary"/>
		<rdfs:comment xml:lang="en">JavaLibrary implementing the java.lang.reflect package for personaljava-1_1</rdfs:comment>
	</owl:Class>
	<owl:Class rdf:about="&personaljava-1_1;JavaIoLibrary">
		<rdfs:subClassOf rdf:resource="&j2me-midp-1_0;JavaIoLibrary"/>
		<rdfs:seeAlso rdf:resource="&personaljava-1_1;JavaUtilLibrary"/>
		<rdfs:seeAlso rdf:resource="&personaljava-1_1;JavaLangLibrary"/>
		<rdfs:comment xml:lang="en">JavaLibrary implementing the java.io package for personaljava-1_1</rdfs:comment>
	</owl:Class>
	<owl:Class rdf:about="&personaljava-1_1;JavaUtilLibrary">
		<rdfs:subClassOf rdf:resource="&java;JavaLibrary"/>
		<rdfs:seeAlso rdf:resource="&personaljava-1_1;JavaLangLibrary"/>
		<rdfs:seeAlso rdf:resource="&personaljava-1_1;JavaIoLibrary"/>
		<rdfs:comment xml:lang="en">JavaLibrary implementing the java.util package for personaljava-1_1</rdfs:comment>
	</owl:Class>
	<owl:Class rdf:about="&personaljava-1_1;JavaUtilZipLibrary">
		<rdfs:subClassOf rdf:resource="&java;JavaLibrary"/>
		<rdfs:seeAlso rdf:resource="&personaljava-1_1;JavaLangLibrary"/>
		<rdfs:seeAlso rdf:resource="&personaljava-1_1;JavaIoLibrary"/>
		<rdfs:comment xml:lang="en">JavaLibrary implementing the java.util.zip package for personaljava-1_1</rdfs:comment>
	</owl:Class>
	<owl:Class rdf:about="&personaljava-1_1;JavaTextLibrary">
		<rdfs:subClassOf rdf:resource="&java;JavaLibrary"/>
		<rdfs:seeAlso rdf:resource="&personaljava-1_1;JavaUtilLibrary"/>
		<rdfs:seeAlso rdf:resource="&personaljava-1_1;JavaLangLibrary"/>
		<rdfs:seeAlso rdf:resource="&personaljava-1_1;JavaIoLibrary"/>
		<rdfs:comment xml:lang="en">JavaLibrary implementing the java.text package for personaljava-1_1</rdfs:comment>
	</owl:Class>
	<owl:Class rdf:about="&personaljava-1_1;JavaTextResourcesLibrary">
		<rdfs:subClassOf rdf:resource="&java;JavaLibrary"/>
		<rdfs:seeAlso rdf:resource="&personaljava-1_1;JavaUtilLibrary"/>
		<rdfs:seeAlso rdf:resource="&personaljava-1_1;JavaLangLibrary"/>
		<rdfs:comment xml:lang="en">JavaLibrary implementing the java.text.resources package for personaljava-1_1</rdfs:comment>
	</owl:Class>
	<owl:Class rdf:about="&personaljava-1_1;JavaNetLibrary">
		<rdfs:subClassOf rdf:resource="&java;JavaLibrary"/>
		<rdfs:seeAlso rdf:resource="&personaljava-1_1;JavaLangLibrary"/>
		<rdfs:seeAlso rdf:resource="&personaljava-1_1;JavaIoLibrary"/>
		<rdfs:comment xml:lang="en">JavaLibrary implementing the java.net package for personaljava-1_1</rdfs:comment>
	</owl:Class>
	<owl:Class rdf:about="&personaljava-1_1;JavaAwtLibrary">
		<rdfs:subClassOf rdf:resource="&java;JavaLibrary"/>
		<rdfs:seeAlso rdf:resource="&personaljava-1_1;JavaUtilLibrary"/>
		<rdfs:seeAlso rdf:resource="&personaljava-1_1;JavaLangLibrary"/>
		<rdfs:seeAlso rdf:resource="&personaljava-1_1;JavaAwtPeerLibrary"/>
		<rdfs:seeAlso rdf:resource="&personaljava-1_1;JavaNetLibrary"/>
		<rdfs:seeAlso rdf:resource="&personaljava-1_1;JavaAwtEventLibrary"/>
		<rdfs:seeAlso rdf:resource="&personaljava-1_1;JavaIoLibrary"/>
		<rdfs:seeAlso rdf:resource="&personaljava-1_1;JavaAwtDatatransferLibrary"/>
		<rdfs:seeAlso rdf:resource="&personaljava-1_1;JavaAwtImageLibrary"/>
		<rdfs:comment xml:lang="en">JavaLibrary implementing the java.awt package for personaljava-1_1</rdfs:comment>
	</owl:Class>
	<owl:Class rdf:about="&personaljava-1_1;JavaAwtImageLibrary">
		<rdfs:subClassOf rdf:resource="&java;JavaLibrary"/>
		<rdfs:seeAlso rdf:resource="&personaljava-1_1;JavaAwtLibrary"/>
		<rdfs:seeAlso rdf:resource="&personaljava-1_1;JavaUtilLibrary"/>
		<rdfs:seeAlso rdf:resource="&personaljava-1_1;JavaLangLibrary"/>
		<rdfs:comment xml:lang="en">JavaLibrary implementing the java.awt.image package for personaljava-1_1</rdfs:comment>
	</owl:Class>
	<owl:Class rdf:about="&personaljava-1_1;JavaAwtEventLibrary">
		<rdfs:subClassOf rdf:resource="&java;JavaLibrary"/>
		<rdfs:seeAlso rdf:resource="&personaljava-1_1;JavaAwtLibrary"/>
		<rdfs:seeAlso rdf:resource="&personaljava-1_1;JavaUtilLibrary"/>
		<rdfs:seeAlso rdf:resource="&personaljava-1_1;JavaLangLibrary"/>
		<rdfs:comment xml:lang="en">JavaLibrary implementing the java.awt.event package for personaljava-1_1</rdfs:comment>
	</owl:Class>
	<owl:Class rdf:about="&personaljava-1_1;JavaAwtPeerLibrary">
		<rdfs:subClassOf rdf:resource="&java;JavaLibrary"/>
		<rdfs:seeAlso rdf:resource="&personaljava-1_1;JavaAwtLibrary"/>
		<rdfs:seeAlso rdf:resource="&personaljava-1_1;JavaLangLibrary"/>
		<rdfs:seeAlso rdf:resource="&personaljava-1_1;JavaAwtImageLibrary"/>
		<rdfs:comment xml:lang="en">JavaLibrary implementing the java.awt.peer package for personaljava-1_1</rdfs:comment>
	</owl:Class>
	<owl:Class rdf:about="&personaljava-1_1;JavaAwtDatatransferLibrary">
		<rdfs:subClassOf rdf:resource="&java;JavaLibrary"/>
		<rdfs:seeAlso rdf:resource="&personaljava-1_1;JavaLangLibrary"/>
		<rdfs:comment xml:lang="en">JavaLibrary implementing the java.awt.datatransfer package for personaljava-1_1</rdfs:comment>
	</owl:Class>
	<owl:Class rdf:about="&personaljava-1_1;JavaAppletLibrary">
		<rdfs:subClassOf rdf:resource="&java;JavaLibrary"/>
		<rdfs:seeAlso rdf:resource="&personaljava-1_1;JavaAwtLibrary"/>
		<rdfs:seeAlso rdf:resource="&personaljava-1_1;JavaUtilLibrary"/>
		<rdfs:seeAlso rdf:resource="&personaljava-1_1;JavaLangLibrary"/>
		<rdfs:seeAlso rdf:resource="&personaljava-1_1;JavaNetLibrary"/>
		<rdfs:comment xml:lang="en">JavaLibrary implementing the java.applet package for personaljava-1_1</rdfs:comment>
	</owl:Class>
	<owl:Class rdf:about="&personaljava-1_1;JavaBeansLibrary">
		<rdfs:subClassOf rdf:resource="&java;JavaLibrary"/>
		<rdfs:seeAlso rdf:resource="&personaljava-1_1;JavaAwtLibrary"/>
		<rdfs:seeAlso rdf:resource="&personaljava-1_1;JavaLangReflectLibrary"/>
		<rdfs:seeAlso rdf:resource="&personaljava-1_1;JavaUtilLibrary"/>
		<rdfs:seeAlso rdf:resource="&personaljava-1_1;JavaIoLibrary"/>
		<rdfs:seeAlso rdf:resource="&personaljava-1_1;JavaLangLibrary"/>
		<rdfs:comment xml:lang="en">JavaLibrary implementing the java.beans package for personaljava-1_1</rdfs:comment>
	</owl:Class>
</rdf:RDF>
