<?xml version="1.0" encoding="ISO-8859-1"?>
<!DOCTYPE rdf:RDF [
	<!ENTITY xsd "http://www.w3.org/2001/XMLSchema#">
	<!ENTITY java "http://soft.vub.ac.be/platformkit/2010/1/java.owl#">
	<!ENTITY j2me-pp-1_1 "http://soft.vub.ac.be/platformkit/2010/1/j2me-pp-1_1.owl#">
	<!ENTITY isa "http://soft.vub.ac.be/platformkit/2010/1/isa.owl#">
	<!ENTITY platform "http://soft.vub.ac.be/platformkit/2010/1/platform.owl#">
	<!ENTITY j2se-1_3 "http://soft.vub.ac.be/platformkit/2010/1/j2se-1_3.owl#">
	<!ENTITY rdf "http://www.w3.org/1999/02/22-rdf-syntax-ns#">
	<!ENTITY rdfs "http://www.w3.org/2000/01/rdf-schema#">
	<!ENTITY owl "http://www.w3.org/2002/07/owl#">
]>
<rdf:RDF
	 xmlns="http://soft.vub.ac.be/platformkit/2010/1/j2se-1_4.owl#"
	 xml:base="http://soft.vub.ac.be/platformkit/2010/1/j2se-1_4.owl"
	 xmlns:xsd="&xsd;"
	 xmlns:java="&java;"
	 xmlns:j2me-pp-1_1="&j2me-pp-1_1;"
	 xmlns:isa="&isa;"
	 xmlns:platform="&platform;"
	 xmlns:j2se-1_3="&j2se-1_3;"
	 xmlns:rdf="&rdf;"
	 xmlns:rdfs="&rdfs;"
	 xmlns:owl="&owl;"
>

	<owl:Ontology rdf:about="">
		<owl:versionInfo>$Id$</owl:versionInfo>
		<owl:imports rdf:resource="http://soft.vub.ac.be/platformkit/2010/1/platform.owl"/>
		<owl:imports rdf:resource="http://soft.vub.ac.be/platformkit/2010/1/java.owl"/>
		<owl:imports rdf:resource="http://soft.vub.ac.be/platformkit/2010/1/j2se-1_3.owl"/>
		<owl:imports rdf:resource="http://soft.vub.ac.be/platformkit/2010/1/isa.owl"/>
		<owl:imports rdf:resource="http://soft.vub.ac.be/platformkit/2010/1/j2me-pp-1_1.owl"/>
		<rdfs:comment xml:lang="en">Generated by [UML2ToSimplifiedPackageAPIOntology.atl 8080 2010-03-18 10:46:40Z dwagelaa], [UML2ToPackageAPIOntology.atl 8082 2010-03-18 21:11:00Z dwagelaa], [UML2ToAPIOntology.atl 8082 2010-03-18 21:11:00Z dwagelaa], and [UML2Comparison.atl 8082 2010-03-18 21:11:00Z dwagelaa]</rdfs:comment>
		<rdfs:comment>Dennis Wagelaar &lt;dennis.wagelaar@vub.ac.be&gt;</rdfs:comment>
		<rdfs:comment xml:lang="en">&#169; 2010, Vrije Universiteit Brussel. All rights reserved.</rdfs:comment>
		<rdfs:label xml:lang="en">J2SE 1.4</rdfs:label>
	</owl:Ontology>
	<owl:Class rdf:about="#J2SE1_4API">
		<rdfs:subClassOf rdf:resource="#JavaLangAPI"/>
		<rdfs:subClassOf rdf:resource="#JavaLangReflectAPI"/>
		<rdfs:subClassOf rdf:resource="#JavaLangRefAPI"/>
		<rdfs:subClassOf rdf:resource="#JavaIoAPI"/>
		<rdfs:subClassOf rdf:resource="#JavaUtilAPI"/>
		<rdfs:subClassOf rdf:resource="#JavaUtilLoggingAPI"/>
		<rdfs:subClassOf rdf:resource="#JavaUtilJarAPI"/>
		<rdfs:subClassOf rdf:resource="#JavaUtilZipAPI"/>
		<rdfs:subClassOf rdf:resource="#JavaUtilPrefsAPI"/>
		<rdfs:subClassOf rdf:resource="#JavaUtilRegexAPI"/>
		<rdfs:subClassOf rdf:resource="#JavaNetAPI"/>
		<rdfs:subClassOf rdf:resource="#JavaSecurityAPI"/>
		<rdfs:subClassOf rdf:resource="#JavaSecurityCertAPI"/>
		<rdfs:subClassOf rdf:resource="#JavaSecuritySpecAPI"/>
		<rdfs:subClassOf rdf:resource="#JavaSecurityAclAPI"/>
		<rdfs:subClassOf rdf:resource="#JavaSecurityInterfacesAPI"/>
		<rdfs:subClassOf rdf:resource="#JavaNioAPI"/>
		<rdfs:subClassOf rdf:resource="#JavaNioChannelsAPI"/>
		<rdfs:subClassOf rdf:resource="#JavaNioChannelsSpiAPI"/>
		<rdfs:subClassOf rdf:resource="#JavaNioCharsetAPI"/>
		<rdfs:subClassOf rdf:resource="#JavaNioCharsetSpiAPI"/>
		<rdfs:subClassOf rdf:resource="#JavaBeansAPI"/>
		<rdfs:subClassOf rdf:resource="#JavaBeansBeancontextAPI"/>
		<rdfs:subClassOf rdf:resource="#JavaAwtAPI"/>
		<rdfs:subClassOf rdf:resource="#JavaAwtImageAPI"/>
		<rdfs:subClassOf rdf:resource="#JavaAwtImageRenderableAPI"/>
		<rdfs:subClassOf rdf:resource="#JavaAwtDatatransferAPI"/>
		<rdfs:subClassOf rdf:resource="#JavaAwtDndAPI"/>
		<rdfs:subClassOf rdf:resource="#JavaAwtEventAPI"/>
		<rdfs:subClassOf rdf:resource="#JavaAwtImAPI"/>
		<rdfs:subClassOf rdf:resource="#JavaAwtImSpiAPI"/>
		<rdfs:subClassOf rdf:resource="#JavaAwtFontAPI"/>
		<rdfs:subClassOf rdf:resource="#JavaAwtGeomAPI"/>
		<rdfs:subClassOf rdf:resource="#JavaAwtColorAPI"/>
		<rdfs:subClassOf rdf:resource="#JavaAwtPrintAPI"/>
		<rdfs:subClassOf rdf:resource="#JavaTextAPI"/>
		<rdfs:subClassOf rdf:resource="#JavaMathAPI"/>
		<rdfs:subClassOf rdf:resource="#JavaAppletAPI"/>
		<rdfs:subClassOf rdf:resource="#JavaRmiAPI"/>
		<rdfs:subClassOf rdf:resource="#JavaRmiActivationAPI"/>
		<rdfs:subClassOf rdf:resource="#JavaRmiServerAPI"/>
		<rdfs:subClassOf rdf:resource="#JavaRmiDgcAPI"/>
		<rdfs:subClassOf rdf:resource="#JavaRmiRegistryAPI"/>
		<rdfs:subClassOf rdf:resource="#JavaSqlAPI"/>
		<rdfs:subClassOf rdf:resource="#JavaxImageioAPI"/>
		<rdfs:subClassOf rdf:resource="#JavaxImageioSpiAPI"/>
		<rdfs:subClassOf rdf:resource="#JavaxImageioMetadataAPI"/>
		<rdfs:subClassOf rdf:resource="#JavaxImageioStreamAPI"/>
		<rdfs:subClassOf rdf:resource="#JavaxImageioEventAPI"/>
		<rdfs:subClassOf rdf:resource="#JavaxImageioPluginsJpegAPI"/>
		<rdfs:subClassOf rdf:resource="#JavaxAccessibilityAPI"/>
		<rdfs:subClassOf rdf:resource="#JavaxSwingAPI"/>
		<rdfs:subClassOf rdf:resource="#JavaxSwingPlafAPI"/>
		<rdfs:subClassOf rdf:resource="#JavaxSwingPlafBasicAPI"/>
		<rdfs:subClassOf rdf:resource="#JavaxSwingPlafMetalAPI"/>
		<rdfs:subClassOf rdf:resource="#JavaxSwingPlafMultiAPI"/>
		<rdfs:subClassOf rdf:resource="#JavaxSwingEventAPI"/>
		<rdfs:subClassOf rdf:resource="#JavaxSwingBorderAPI"/>
		<rdfs:subClassOf rdf:resource="#JavaxSwingTextAPI"/>
		<rdfs:subClassOf rdf:resource="#JavaxSwingTextHtmlAPI"/>
		<rdfs:subClassOf rdf:resource="#JavaxSwingTextHtmlParserAPI"/>
		<rdfs:subClassOf rdf:resource="#JavaxSwingTextRtfAPI"/>
		<rdfs:subClassOf rdf:resource="#JavaxSwingTableAPI"/>
		<rdfs:subClassOf rdf:resource="#JavaxSwingUndoAPI"/>
		<rdfs:subClassOf rdf:resource="#JavaxSwingTreeAPI"/>
		<rdfs:subClassOf rdf:resource="#JavaxSwingFilechooserAPI"/>
		<rdfs:subClassOf rdf:resource="#JavaxSwingColorchooserAPI"/>
		<rdfs:subClassOf rdf:resource="#JavaxSoundSampledAPI"/>
		<rdfs:subClassOf rdf:resource="#JavaxSoundSampledSpiAPI"/>
		<rdfs:subClassOf rdf:resource="#JavaxSoundMidiAPI"/>
		<rdfs:subClassOf rdf:resource="#JavaxSoundMidiSpiAPI"/>
		<rdfs:subClassOf rdf:resource="#JavaxPrintAPI"/>
		<rdfs:subClassOf rdf:resource="#JavaxPrintAttributeAPI"/>
		<rdfs:subClassOf rdf:resource="#JavaxPrintAttributeStandardAPI"/>
		<rdfs:subClassOf rdf:resource="#JavaxPrintEventAPI"/>
		<rdfs:subClassOf rdf:resource="#JavaxSecurityAuthAPI"/>
		<rdfs:subClassOf rdf:resource="#JavaxSecurityAuthX500API"/>
		<rdfs:subClassOf rdf:resource="#JavaxSecurityAuthCallbackAPI"/>
		<rdfs:subClassOf rdf:resource="#JavaxSecurityAuthKerberosAPI"/>
		<rdfs:subClassOf rdf:resource="#JavaxSecurityAuthLoginAPI"/>
		<rdfs:subClassOf rdf:resource="#JavaxSecurityAuthSpiAPI"/>
		<rdfs:subClassOf rdf:resource="#JavaxSecurityCertAPI"/>
		<rdfs:subClassOf rdf:resource="#JavaxNamingAPI"/>
		<rdfs:subClassOf rdf:resource="#JavaxNamingDirectoryAPI"/>
		<rdfs:subClassOf rdf:resource="#JavaxNamingEventAPI"/>
		<rdfs:subClassOf rdf:resource="#JavaxNamingLdapAPI"/>
		<rdfs:subClassOf rdf:resource="#JavaxNamingSpiAPI"/>
		<rdfs:subClassOf rdf:resource="#JavaxNetAPI"/>
		<rdfs:subClassOf rdf:resource="#JavaxNetSslAPI"/>
		<rdfs:subClassOf rdf:resource="#JavaxRmiAPI"/>
		<rdfs:subClassOf rdf:resource="#JavaxRmiCORBAAPI"/>
		<rdfs:subClassOf rdf:resource="#JavaxCryptoAPI"/>
		<rdfs:subClassOf rdf:resource="#JavaxCryptoInterfacesAPI"/>
		<rdfs:subClassOf rdf:resource="#JavaxCryptoSpecAPI"/>
		<rdfs:subClassOf rdf:resource="#JavaxSqlAPI"/>
		<rdfs:subClassOf rdf:resource="#JavaxTransactionAPI"/>
		<rdfs:subClassOf rdf:resource="#JavaxTransactionXaAPI"/>
		<rdfs:subClassOf rdf:resource="#JavaxXmlParsersAPI"/>
		<rdfs:subClassOf rdf:resource="#JavaxXmlTransformAPI"/>
		<rdfs:subClassOf rdf:resource="#JavaxXmlTransformDomAPI"/>
		<rdfs:subClassOf rdf:resource="#JavaxXmlTransformSaxAPI"/>
		<rdfs:subClassOf rdf:resource="#JavaxXmlTransformStreamAPI"/>
		<rdfs:subClassOf rdf:resource="#OrgW3cDomAPI"/>
		<rdfs:subClassOf rdf:resource="#OrgW3cDomCssAPI"/>
		<rdfs:subClassOf rdf:resource="#OrgW3cDomStylesheetsAPI"/>
		<rdfs:subClassOf rdf:resource="#OrgW3cDomViewsAPI"/>
		<rdfs:subClassOf rdf:resource="#OrgW3cDomEventsAPI"/>
		<rdfs:subClassOf rdf:resource="#OrgW3cDomHtmlAPI"/>
		<rdfs:subClassOf rdf:resource="#OrgW3cDomTraversalAPI"/>
		<rdfs:subClassOf rdf:resource="#OrgOmgCORBA_2_3API"/>
		<rdfs:subClassOf rdf:resource="#OrgOmgCORBA_2_3PortableAPI"/>
		<rdfs:subClassOf rdf:resource="#OrgOmgCORBAAPI"/>
		<rdfs:subClassOf rdf:resource="#OrgOmgCORBAPortableAPI"/>
		<rdfs:subClassOf rdf:resource="#OrgOmgCORBADynAnyPackageAPI"/>
		<rdfs:subClassOf rdf:resource="#OrgOmgCORBAORBPackageAPI"/>
		<rdfs:subClassOf rdf:resource="#OrgOmgCORBATypeCodePackageAPI"/>
		<rdfs:subClassOf rdf:resource="#OrgOmgSendingContextAPI"/>
		<rdfs:subClassOf rdf:resource="#OrgOmgCosNamingAPI"/>
		<rdfs:subClassOf rdf:resource="#OrgOmgCosNamingNamingContextExtPackageAPI"/>
		<rdfs:subClassOf rdf:resource="#OrgOmgCosNamingNamingContextPackageAPI"/>
		<rdfs:subClassOf rdf:resource="#OrgOmgPortableServerAPI"/>
		<rdfs:subClassOf rdf:resource="#OrgOmgPortableServerCurrentPackageAPI"/>
		<rdfs:subClassOf rdf:resource="#OrgOmgPortableServerPOAManagerPackageAPI"/>
		<rdfs:subClassOf rdf:resource="#OrgOmgPortableServerPOAPackageAPI"/>
		<rdfs:subClassOf rdf:resource="#OrgOmgPortableServerPortableAPI"/>
		<rdfs:subClassOf rdf:resource="#OrgOmgPortableServerServantLocatorPackageAPI"/>
		<rdfs:subClassOf rdf:resource="#OrgOmgDynamicAPI"/>
		<rdfs:subClassOf rdf:resource="#OrgOmgDynamicAnyAPI"/>
		<rdfs:subClassOf rdf:resource="#OrgOmgDynamicAnyDynAnyFactoryPackageAPI"/>
		<rdfs:subClassOf rdf:resource="#OrgOmgDynamicAnyDynAnyPackageAPI"/>
		<rdfs:subClassOf rdf:resource="#OrgOmgIOPAPI"/>
		<rdfs:subClassOf rdf:resource="#OrgOmgIOPCodecFactoryPackageAPI"/>
		<rdfs:subClassOf rdf:resource="#OrgOmgIOPCodecPackageAPI"/>
		<rdfs:subClassOf rdf:resource="#OrgOmgMessagingAPI"/>
		<rdfs:subClassOf rdf:resource="#OrgOmgPortableInterceptorAPI"/>
		<rdfs:subClassOf rdf:resource="#OrgOmgPortableInterceptorORBInitInfoPackageAPI"/>
		<rdfs:subClassOf rdf:resource="#OrgOmgStubJavaRmiAPI"/>
		<rdfs:subClassOf rdf:resource="#OrgXmlSaxAPI"/>
		<rdfs:subClassOf rdf:resource="#OrgXmlSaxHelpersAPI"/>
		<rdfs:subClassOf rdf:resource="#OrgXmlSaxExtAPI"/>
		<rdfs:subClassOf rdf:resource="#OrgIetfJgssAPI"/>
		<rdfs:comment xml:lang="en">J2SE 1.4 API</rdfs:comment>
		<rdfs:comment xml:lang="OWLManchester">platform:comprisesInterfacePart some JavaLang and platform:comprisesInterfacePart some JavaLangReflect and platform:comprisesInterfacePart some JavaLangRef and platform:comprisesInterfacePart some JavaIo and platform:comprisesInterfacePart some JavaUtil and platform:comprisesInterfacePart some JavaUtilLogging and platform:comprisesInterfacePart some JavaUtilJar and platform:comprisesInterfacePart some JavaUtilZip and platform:comprisesInterfacePart some JavaUtilPrefs and platform:comprisesInterfacePart some JavaUtilRegex and platform:comprisesInterfacePart some JavaNet and platform:comprisesInterfacePart some JavaSecurity and platform:comprisesInterfacePart some JavaSecurityCert and platform:comprisesInterfacePart some JavaSecuritySpec and platform:comprisesInterfacePart some JavaSecurityAcl and platform:comprisesInterfacePart some JavaSecurityInterfaces and platform:comprisesInterfacePart some JavaNio and platform:comprisesInterfacePart some JavaNioChannels and platform:comprisesInterfacePart some JavaNioChannelsSpi and platform:comprisesInterfacePart some JavaNioCharset and platform:comprisesInterfacePart some JavaNioCharsetSpi and platform:comprisesInterfacePart some JavaBeans and platform:comprisesInterfacePart some JavaBeansBeancontext and platform:comprisesInterfacePart some JavaAwt and platform:comprisesInterfacePart some JavaAwtImage and platform:comprisesInterfacePart some JavaAwtImageRenderable and platform:comprisesInterfacePart some JavaAwtDatatransfer and platform:comprisesInterfacePart some JavaAwtDnd and platform:comprisesInterfacePart some JavaAwtEvent and platform:comprisesInterfacePart some JavaAwtIm and platform:comprisesInterfacePart some JavaAwtImSpi and platform:comprisesInterfacePart some JavaAwtFont and platform:comprisesInterfacePart some JavaAwtGeom and platform:comprisesInterfacePart some JavaAwtColor and platform:comprisesInterfacePart some JavaAwtPrint and platform:comprisesInterfacePart some JavaText and platform:comprisesInterfacePart some JavaMath and platform:comprisesInterfacePart some JavaApplet and platform:comprisesInterfacePart some JavaRmi and platform:comprisesInterfacePart some JavaRmiActivation and platform:comprisesInterfacePart some JavaRmiServer and platform:comprisesInterfacePart some JavaRmiDgc and platform:comprisesInterfacePart some JavaRmiRegistry and platform:comprisesInterfacePart some JavaSql and platform:comprisesInterfacePart some JavaxImageio and platform:comprisesInterfacePart some JavaxImageioSpi and platform:comprisesInterfacePart some JavaxImageioMetadata and platform:comprisesInterfacePart some JavaxImageioStream and platform:comprisesInterfacePart some JavaxImageioEvent and platform:comprisesInterfacePart some JavaxImageioPluginsJpeg and platform:comprisesInterfacePart some JavaxAccessibility and platform:comprisesInterfacePart some JavaxSwing and platform:comprisesInterfacePart some JavaxSwingPlaf and platform:comprisesInterfacePart some JavaxSwingPlafBasic and platform:comprisesInterfacePart some JavaxSwingPlafMetal and platform:comprisesInterfacePart some JavaxSwingPlafMulti and platform:comprisesInterfacePart some JavaxSwingEvent and platform:comprisesInterfacePart some JavaxSwingBorder and platform:comprisesInterfacePart some JavaxSwingText and platform:comprisesInterfacePart some JavaxSwingTextHtml and platform:comprisesInterfacePart some JavaxSwingTextHtmlParser and platform:comprisesInterfacePart some JavaxSwingTextRtf and platform:comprisesInterfacePart some JavaxSwingTable and platform:comprisesInterfacePart some JavaxSwingUndo and platform:comprisesInterfacePart some JavaxSwingTree and platform:comprisesInterfacePart some JavaxSwingFilechooser and platform:comprisesInterfacePart some JavaxSwingColorchooser and platform:comprisesInterfacePart some JavaxSoundSampled and platform:comprisesInterfacePart some JavaxSoundSampledSpi and platform:comprisesInterfacePart some JavaxSoundMidi and platform:comprisesInterfacePart some JavaxSoundMidiSpi and platform:comprisesInterfacePart some JavaxPrint and platform:comprisesInterfacePart some JavaxPrintAttribute and platform:comprisesInterfacePart some JavaxPrintAttributeStandard and platform:comprisesInterfacePart some JavaxPrintEvent and platform:comprisesInterfacePart some JavaxSecurityAuth and platform:comprisesInterfacePart some JavaxSecurityAuthX500 and platform:comprisesInterfacePart some JavaxSecurityAuthCallback and platform:comprisesInterfacePart some JavaxSecurityAuthKerberos and platform:comprisesInterfacePart some JavaxSecurityAuthLogin and platform:comprisesInterfacePart some JavaxSecurityAuthSpi and platform:comprisesInterfacePart some JavaxSecurityCert and platform:comprisesInterfacePart some JavaxNaming and platform:comprisesInterfacePart some JavaxNamingDirectory and platform:comprisesInterfacePart some JavaxNamingEvent and platform:comprisesInterfacePart some JavaxNamingLdap and platform:comprisesInterfacePart some JavaxNamingSpi and platform:comprisesInterfacePart some JavaxNet and platform:comprisesInterfacePart some JavaxNetSsl and platform:comprisesInterfacePart some JavaxRmi and platform:comprisesInterfacePart some JavaxRmiCORBA and platform:comprisesInterfacePart some JavaxCrypto and platform:comprisesInterfacePart some JavaxCryptoInterfaces and platform:comprisesInterfacePart some JavaxCryptoSpec and platform:comprisesInterfacePart some JavaxSql and platform:comprisesInterfacePart some JavaxTransaction and platform:comprisesInterfacePart some JavaxTransactionXa and platform:comprisesInterfacePart some JavaxXmlParsers and platform:comprisesInterfacePart some JavaxXmlTransform and platform:comprisesInterfacePart some JavaxXmlTransformDom and platform:comprisesInterfacePart some JavaxXmlTransformSax and platform:comprisesInterfacePart some JavaxXmlTransformStream and platform:comprisesInterfacePart some OrgW3cDom and platform:comprisesInterfacePart some OrgW3cDomCss and platform:comprisesInterfacePart some OrgW3cDomStylesheets and platform:comprisesInterfacePart some OrgW3cDomViews and platform:comprisesInterfacePart some OrgW3cDomEvents and platform:comprisesInterfacePart some OrgW3cDomHtml and platform:comprisesInterfacePart some OrgW3cDomTraversal and platform:comprisesInterfacePart some OrgOmgCORBA_2_3 and platform:comprisesInterfacePart some OrgOmgCORBA_2_3Portable and platform:comprisesInterfacePart some OrgOmgCORBA and platform:comprisesInterfacePart some OrgOmgCORBAPortable and platform:comprisesInterfacePart some OrgOmgCORBADynAnyPackage and platform:comprisesInterfacePart some OrgOmgCORBAORBPackage and platform:comprisesInterfacePart some OrgOmgCORBATypeCodePackage and platform:comprisesInterfacePart some OrgOmgSendingContext and platform:comprisesInterfacePart some OrgOmgCosNaming and platform:comprisesInterfacePart some OrgOmgCosNamingNamingContextExtPackage and platform:comprisesInterfacePart some OrgOmgCosNamingNamingContextPackage and platform:comprisesInterfacePart some OrgOmgPortableServer and platform:comprisesInterfacePart some OrgOmgPortableServerCurrentPackage and platform:comprisesInterfacePart some OrgOmgPortableServerPOAManagerPackage and platform:comprisesInterfacePart some OrgOmgPortableServerPOAPackage and platform:comprisesInterfacePart some OrgOmgPortableServerPortable and platform:comprisesInterfacePart some OrgOmgPortableServerServantLocatorPackage and platform:comprisesInterfacePart some OrgOmgDynamic and platform:comprisesInterfacePart some OrgOmgDynamicAny and platform:comprisesInterfacePart some OrgOmgDynamicAnyDynAnyFactoryPackage and platform:comprisesInterfacePart some OrgOmgDynamicAnyDynAnyPackage and platform:comprisesInterfacePart some OrgOmgIOP and platform:comprisesInterfacePart some OrgOmgIOPCodecFactoryPackage and platform:comprisesInterfacePart some OrgOmgIOPCodecPackage and platform:comprisesInterfacePart some OrgOmgMessaging and platform:comprisesInterfacePart some OrgOmgPortableInterceptor and platform:comprisesInterfacePart some OrgOmgPortableInterceptorORBInitInfoPackage and platform:comprisesInterfacePart some OrgOmgStubJavaRmi and platform:comprisesInterfacePart some OrgXmlSax and platform:comprisesInterfacePart some OrgXmlSaxHelpers and platform:comprisesInterfacePart some OrgXmlSaxExt and platform:comprisesInterfacePart some OrgIetfJgss</rdfs:comment>
	</owl:Class>
	<owl:Class rdf:about="#J2SE1_4ClassLibrary">
		<rdfs:subClassOf rdf:resource="#JavaLangClassLibrary"/>
		<rdfs:subClassOf rdf:resource="#JavaLangReflectClassLibrary"/>
		<rdfs:subClassOf rdf:resource="#JavaLangRefClassLibrary"/>
		<rdfs:subClassOf rdf:resource="#JavaIoClassLibrary"/>
		<rdfs:subClassOf rdf:resource="#JavaUtilClassLibrary"/>
		<rdfs:subClassOf rdf:resource="#JavaUtilLoggingClassLibrary"/>
		<rdfs:subClassOf rdf:resource="#JavaUtilJarClassLibrary"/>
		<rdfs:subClassOf rdf:resource="#JavaUtilZipClassLibrary"/>
		<rdfs:subClassOf rdf:resource="#JavaUtilPrefsClassLibrary"/>
		<rdfs:subClassOf rdf:resource="#JavaUtilRegexClassLibrary"/>
		<rdfs:subClassOf rdf:resource="#JavaNetClassLibrary"/>
		<rdfs:subClassOf rdf:resource="#JavaSecurityClassLibrary"/>
		<rdfs:subClassOf rdf:resource="#JavaSecurityCertClassLibrary"/>
		<rdfs:subClassOf rdf:resource="#JavaSecuritySpecClassLibrary"/>
		<rdfs:subClassOf rdf:resource="#JavaSecurityAclClassLibrary"/>
		<rdfs:subClassOf rdf:resource="#JavaSecurityInterfacesClassLibrary"/>
		<rdfs:subClassOf rdf:resource="#JavaNioClassLibrary"/>
		<rdfs:subClassOf rdf:resource="#JavaNioChannelsClassLibrary"/>
		<rdfs:subClassOf rdf:resource="#JavaNioChannelsSpiClassLibrary"/>
		<rdfs:subClassOf rdf:resource="#JavaNioCharsetClassLibrary"/>
		<rdfs:subClassOf rdf:resource="#JavaNioCharsetSpiClassLibrary"/>
		<rdfs:subClassOf rdf:resource="#JavaBeansClassLibrary"/>
		<rdfs:subClassOf rdf:resource="#JavaBeansBeancontextClassLibrary"/>
		<rdfs:subClassOf rdf:resource="#JavaAwtClassLibrary"/>
		<rdfs:subClassOf rdf:resource="#JavaAwtImageClassLibrary"/>
		<rdfs:subClassOf rdf:resource="#JavaAwtImageRenderableClassLibrary"/>
		<rdfs:subClassOf rdf:resource="#JavaAwtDatatransferClassLibrary"/>
		<rdfs:subClassOf rdf:resource="#JavaAwtDndClassLibrary"/>
		<rdfs:subClassOf rdf:resource="#JavaAwtEventClassLibrary"/>
		<rdfs:subClassOf rdf:resource="#JavaAwtImClassLibrary"/>
		<rdfs:subClassOf rdf:resource="#JavaAwtImSpiClassLibrary"/>
		<rdfs:subClassOf rdf:resource="#JavaAwtFontClassLibrary"/>
		<rdfs:subClassOf rdf:resource="#JavaAwtGeomClassLibrary"/>
		<rdfs:subClassOf rdf:resource="#JavaAwtColorClassLibrary"/>
		<rdfs:subClassOf rdf:resource="#JavaAwtPrintClassLibrary"/>
		<rdfs:subClassOf rdf:resource="#JavaTextClassLibrary"/>
		<rdfs:subClassOf rdf:resource="#JavaMathClassLibrary"/>
		<rdfs:subClassOf rdf:resource="#JavaAppletClassLibrary"/>
		<rdfs:subClassOf rdf:resource="#JavaRmiClassLibrary"/>
		<rdfs:subClassOf rdf:resource="#JavaRmiActivationClassLibrary"/>
		<rdfs:subClassOf rdf:resource="#JavaRmiServerClassLibrary"/>
		<rdfs:subClassOf rdf:resource="#JavaRmiDgcClassLibrary"/>
		<rdfs:subClassOf rdf:resource="#JavaRmiRegistryClassLibrary"/>
		<rdfs:subClassOf rdf:resource="#JavaSqlClassLibrary"/>
		<rdfs:subClassOf rdf:resource="#JavaxImageioClassLibrary"/>
		<rdfs:subClassOf rdf:resource="#JavaxImageioSpiClassLibrary"/>
		<rdfs:subClassOf rdf:resource="#JavaxImageioMetadataClassLibrary"/>
		<rdfs:subClassOf rdf:resource="#JavaxImageioStreamClassLibrary"/>
		<rdfs:subClassOf rdf:resource="#JavaxImageioEventClassLibrary"/>
		<rdfs:subClassOf rdf:resource="#JavaxImageioPluginsJpegClassLibrary"/>
		<rdfs:subClassOf rdf:resource="#JavaxAccessibilityClassLibrary"/>
		<rdfs:subClassOf rdf:resource="#JavaxSwingClassLibrary"/>
		<rdfs:subClassOf rdf:resource="#JavaxSwingPlafClassLibrary"/>
		<rdfs:subClassOf rdf:resource="#JavaxSwingPlafBasicClassLibrary"/>
		<rdfs:subClassOf rdf:resource="#JavaxSwingPlafMetalClassLibrary"/>
		<rdfs:subClassOf rdf:resource="#JavaxSwingPlafMultiClassLibrary"/>
		<rdfs:subClassOf rdf:resource="#JavaxSwingEventClassLibrary"/>
		<rdfs:subClassOf rdf:resource="#JavaxSwingBorderClassLibrary"/>
		<rdfs:subClassOf rdf:resource="#JavaxSwingTextClassLibrary"/>
		<rdfs:subClassOf rdf:resource="#JavaxSwingTextHtmlClassLibrary"/>
		<rdfs:subClassOf rdf:resource="#JavaxSwingTextHtmlParserClassLibrary"/>
		<rdfs:subClassOf rdf:resource="#JavaxSwingTextRtfClassLibrary"/>
		<rdfs:subClassOf rdf:resource="#JavaxSwingTableClassLibrary"/>
		<rdfs:subClassOf rdf:resource="#JavaxSwingUndoClassLibrary"/>
		<rdfs:subClassOf rdf:resource="#JavaxSwingTreeClassLibrary"/>
		<rdfs:subClassOf rdf:resource="#JavaxSwingFilechooserClassLibrary"/>
		<rdfs:subClassOf rdf:resource="#JavaxSwingColorchooserClassLibrary"/>
		<rdfs:subClassOf rdf:resource="#JavaxSoundSampledClassLibrary"/>
		<rdfs:subClassOf rdf:resource="#JavaxSoundSampledSpiClassLibrary"/>
		<rdfs:subClassOf rdf:resource="#JavaxSoundMidiClassLibrary"/>
		<rdfs:subClassOf rdf:resource="#JavaxSoundMidiSpiClassLibrary"/>
		<rdfs:subClassOf rdf:resource="#JavaxPrintClassLibrary"/>
		<rdfs:subClassOf rdf:resource="#JavaxPrintAttributeClassLibrary"/>
		<rdfs:subClassOf rdf:resource="#JavaxPrintAttributeStandardClassLibrary"/>
		<rdfs:subClassOf rdf:resource="#JavaxPrintEventClassLibrary"/>
		<rdfs:subClassOf rdf:resource="#JavaxSecurityAuthClassLibrary"/>
		<rdfs:subClassOf rdf:resource="#JavaxSecurityAuthX500ClassLibrary"/>
		<rdfs:subClassOf rdf:resource="#JavaxSecurityAuthCallbackClassLibrary"/>
		<rdfs:subClassOf rdf:resource="#JavaxSecurityAuthKerberosClassLibrary"/>
		<rdfs:subClassOf rdf:resource="#JavaxSecurityAuthLoginClassLibrary"/>
		<rdfs:subClassOf rdf:resource="#JavaxSecurityAuthSpiClassLibrary"/>
		<rdfs:subClassOf rdf:resource="#JavaxSecurityCertClassLibrary"/>
		<rdfs:subClassOf rdf:resource="#JavaxNamingClassLibrary"/>
		<rdfs:subClassOf rdf:resource="#JavaxNamingDirectoryClassLibrary"/>
		<rdfs:subClassOf rdf:resource="#JavaxNamingEventClassLibrary"/>
		<rdfs:subClassOf rdf:resource="#JavaxNamingLdapClassLibrary"/>
		<rdfs:subClassOf rdf:resource="#JavaxNamingSpiClassLibrary"/>
		<rdfs:subClassOf rdf:resource="#JavaxNetClassLibrary"/>
		<rdfs:subClassOf rdf:resource="#JavaxNetSslClassLibrary"/>
		<rdfs:subClassOf rdf:resource="#JavaxRmiClassLibrary"/>
		<rdfs:subClassOf rdf:resource="#JavaxRmiCORBAClassLibrary"/>
		<rdfs:subClassOf rdf:resource="#JavaxCryptoClassLibrary"/>
		<rdfs:subClassOf rdf:resource="#JavaxCryptoInterfacesClassLibrary"/>
		<rdfs:subClassOf rdf:resource="#JavaxCryptoSpecClassLibrary"/>
		<rdfs:subClassOf rdf:resource="#JavaxSqlClassLibrary"/>
		<rdfs:subClassOf rdf:resource="#JavaxTransactionClassLibrary"/>
		<rdfs:subClassOf rdf:resource="#JavaxTransactionXaClassLibrary"/>
		<rdfs:subClassOf rdf:resource="#JavaxXmlParsersClassLibrary"/>
		<rdfs:subClassOf rdf:resource="#JavaxXmlTransformClassLibrary"/>
		<rdfs:subClassOf rdf:resource="#JavaxXmlTransformDomClassLibrary"/>
		<rdfs:subClassOf rdf:resource="#JavaxXmlTransformSaxClassLibrary"/>
		<rdfs:subClassOf rdf:resource="#JavaxXmlTransformStreamClassLibrary"/>
		<rdfs:subClassOf rdf:resource="#OrgW3cDomClassLibrary"/>
		<rdfs:subClassOf rdf:resource="#OrgW3cDomCssClassLibrary"/>
		<rdfs:subClassOf rdf:resource="#OrgW3cDomStylesheetsClassLibrary"/>
		<rdfs:subClassOf rdf:resource="#OrgW3cDomViewsClassLibrary"/>
		<rdfs:subClassOf rdf:resource="#OrgW3cDomEventsClassLibrary"/>
		<rdfs:subClassOf rdf:resource="#OrgW3cDomHtmlClassLibrary"/>
		<rdfs:subClassOf rdf:resource="#OrgW3cDomTraversalClassLibrary"/>
		<rdfs:subClassOf rdf:resource="#OrgOmgCORBA_2_3ClassLibrary"/>
		<rdfs:subClassOf rdf:resource="#OrgOmgCORBA_2_3PortableClassLibrary"/>
		<rdfs:subClassOf rdf:resource="#OrgOmgCORBAClassLibrary"/>
		<rdfs:subClassOf rdf:resource="#OrgOmgCORBAPortableClassLibrary"/>
		<rdfs:subClassOf rdf:resource="#OrgOmgCORBADynAnyPackageClassLibrary"/>
		<rdfs:subClassOf rdf:resource="#OrgOmgCORBAORBPackageClassLibrary"/>
		<rdfs:subClassOf rdf:resource="#OrgOmgCORBATypeCodePackageClassLibrary"/>
		<rdfs:subClassOf rdf:resource="#OrgOmgSendingContextClassLibrary"/>
		<rdfs:subClassOf rdf:resource="#OrgOmgCosNamingClassLibrary"/>
		<rdfs:subClassOf rdf:resource="#OrgOmgCosNamingNamingContextExtPackageClassLibrary"/>
		<rdfs:subClassOf rdf:resource="#OrgOmgCosNamingNamingContextPackageClassLibrary"/>
		<rdfs:subClassOf rdf:resource="#OrgOmgPortableServerClassLibrary"/>
		<rdfs:subClassOf rdf:resource="#OrgOmgPortableServerCurrentPackageClassLibrary"/>
		<rdfs:subClassOf rdf:resource="#OrgOmgPortableServerPOAManagerPackageClassLibrary"/>
		<rdfs:subClassOf rdf:resource="#OrgOmgPortableServerPOAPackageClassLibrary"/>
		<rdfs:subClassOf rdf:resource="#OrgOmgPortableServerPortableClassLibrary"/>
		<rdfs:subClassOf rdf:resource="#OrgOmgPortableServerServantLocatorPackageClassLibrary"/>
		<rdfs:subClassOf rdf:resource="#OrgOmgDynamicClassLibrary"/>
		<rdfs:subClassOf rdf:resource="#OrgOmgDynamicAnyClassLibrary"/>
		<rdfs:subClassOf rdf:resource="#OrgOmgDynamicAnyDynAnyFactoryPackageClassLibrary"/>
		<rdfs:subClassOf rdf:resource="#OrgOmgDynamicAnyDynAnyPackageClassLibrary"/>
		<rdfs:subClassOf rdf:resource="#OrgOmgIOPClassLibrary"/>
		<rdfs:subClassOf rdf:resource="#OrgOmgIOPCodecFactoryPackageClassLibrary"/>
		<rdfs:subClassOf rdf:resource="#OrgOmgIOPCodecPackageClassLibrary"/>
		<rdfs:subClassOf rdf:resource="#OrgOmgMessagingClassLibrary"/>
		<rdfs:subClassOf rdf:resource="#OrgOmgPortableInterceptorClassLibrary"/>
		<rdfs:subClassOf rdf:resource="#OrgOmgPortableInterceptorORBInitInfoPackageClassLibrary"/>
		<rdfs:subClassOf rdf:resource="#OrgOmgStubJavaRmiClassLibrary"/>
		<rdfs:subClassOf rdf:resource="#OrgXmlSaxClassLibrary"/>
		<rdfs:subClassOf rdf:resource="#OrgXmlSaxHelpersClassLibrary"/>
		<rdfs:subClassOf rdf:resource="#OrgXmlSaxExtClassLibrary"/>
		<rdfs:subClassOf rdf:resource="#OrgIetfJgssClassLibrary"/>
		<rdfs:comment xml:lang="en">Java class library implementing the J2SE 1.4 API</rdfs:comment>
		<rdfs:comment xml:lang="OWLManchester">platform:implementsInterface some J2SE1_4API</rdfs:comment>
	</owl:Class>
	<owl:Class rdf:about="#J2SE1_4BytecodeFormat">
		<owl:equivalentClass rdf:resource="&j2me-pp-1_1;J2MEPP1_1BytecodeFormat"/>
		<rdfs:subClassOf rdf:resource="&j2se-1_3;J2SE1_3BytecodeFormat"/>
		<rdfs:comment xml:lang="en">J2SE 1.4 bytecode format</rdfs:comment>
		<rdfs:comment xml:lang="OWLManchester">java:majorVersionNumber some xsd:integer[>="48"^^xsd:integer] and java:preverified value false</rdfs:comment>
	</owl:Class>
	<J2SE1_4BytecodeFormat rdf:about="#theJ2SE1_4BytecodeFormat">
		<java:preverified rdf:datatype="http://www.w3.org/2001/XMLSchema#boolean">false</java:preverified>
		<java:minorVersionNumber rdf:datatype="http://www.w3.org/2001/XMLSchema#integer">3</java:minorVersionNumber>
		<java:majorVersionNumber rdf:datatype="http://www.w3.org/2001/XMLSchema#integer">48</java:majorVersionNumber>
	</J2SE1_4BytecodeFormat>
	<J2SE1_4API rdf:about="#theJ2SE1_4API">
		<platform:comprisesInterfacePart rdf:resource="#theOrgIetfJgssPart"/>
		<platform:comprisesInterfacePart rdf:resource="#theOrgXmlSaxExtPart"/>
		<platform:comprisesInterfacePart rdf:resource="#theOrgXmlSaxHelpersPart"/>
		<platform:comprisesInterfacePart rdf:resource="#theOrgXmlSaxPart"/>
		<platform:comprisesInterfacePart rdf:resource="#theOrgOmgStubJavaRmiPart"/>
		<platform:comprisesInterfacePart rdf:resource="#theOrgOmgPortableInterceptorORBInitInfoPackagePart"/>
		<platform:comprisesInterfacePart rdf:resource="#theOrgOmgPortableInterceptorPart"/>
		<platform:comprisesInterfacePart rdf:resource="#theOrgOmgMessagingPart"/>
		<platform:comprisesInterfacePart rdf:resource="#theOrgOmgIOPCodecPackagePart"/>
		<platform:comprisesInterfacePart rdf:resource="#theOrgOmgIOPCodecFactoryPackagePart"/>
		<platform:comprisesInterfacePart rdf:resource="#theOrgOmgIOPPart"/>
		<platform:comprisesInterfacePart rdf:resource="#theOrgOmgDynamicAnyDynAnyPackagePart"/>
		<platform:comprisesInterfacePart rdf:resource="#theOrgOmgDynamicAnyDynAnyFactoryPackagePart"/>
		<platform:comprisesInterfacePart rdf:resource="#theOrgOmgDynamicAnyPart"/>
		<platform:comprisesInterfacePart rdf:resource="#theOrgOmgDynamicPart"/>
		<platform:comprisesInterfacePart rdf:resource="#theOrgOmgPortableServerServantLocatorPackagePart"/>
		<platform:comprisesInterfacePart rdf:resource="#theOrgOmgPortableServerPortablePart"/>
		<platform:comprisesInterfacePart rdf:resource="#theOrgOmgPortableServerPOAPackagePart"/>
		<platform:comprisesInterfacePart rdf:resource="#theOrgOmgPortableServerPOAManagerPackagePart"/>
		<platform:comprisesInterfacePart rdf:resource="#theOrgOmgPortableServerCurrentPackagePart"/>
		<platform:comprisesInterfacePart rdf:resource="#theOrgOmgPortableServerPart"/>
		<platform:comprisesInterfacePart rdf:resource="#theOrgOmgCosNamingNamingContextPackagePart"/>
		<platform:comprisesInterfacePart rdf:resource="#theOrgOmgCosNamingNamingContextExtPackagePart"/>
		<platform:comprisesInterfacePart rdf:resource="#theOrgOmgCosNamingPart"/>
		<platform:comprisesInterfacePart rdf:resource="#theOrgOmgSendingContextPart"/>
		<platform:comprisesInterfacePart rdf:resource="#theOrgOmgCORBATypeCodePackagePart"/>
		<platform:comprisesInterfacePart rdf:resource="#theOrgOmgCORBAORBPackagePart"/>
		<platform:comprisesInterfacePart rdf:resource="#theOrgOmgCORBADynAnyPackagePart"/>
		<platform:comprisesInterfacePart rdf:resource="#theOrgOmgCORBAPortablePart"/>
		<platform:comprisesInterfacePart rdf:resource="#theOrgOmgCORBAPart"/>
		<platform:comprisesInterfacePart rdf:resource="#theOrgOmgCORBA_2_3PortablePart"/>
		<platform:comprisesInterfacePart rdf:resource="#theOrgOmgCORBA_2_3Part"/>
		<platform:comprisesInterfacePart rdf:resource="#theOrgW3cDomTraversalPart"/>
		<platform:comprisesInterfacePart rdf:resource="#theOrgW3cDomHtmlPart"/>
		<platform:comprisesInterfacePart rdf:resource="#theOrgW3cDomEventsPart"/>
		<platform:comprisesInterfacePart rdf:resource="#theOrgW3cDomViewsPart"/>
		<platform:comprisesInterfacePart rdf:resource="#theOrgW3cDomStylesheetsPart"/>
		<platform:comprisesInterfacePart rdf:resource="#theOrgW3cDomCssPart"/>
		<platform:comprisesInterfacePart rdf:resource="#theOrgW3cDomPart"/>
		<platform:comprisesInterfacePart rdf:resource="#theJavaxXmlTransformStreamPart"/>
		<platform:comprisesInterfacePart rdf:resource="#theJavaxXmlTransformSaxPart"/>
		<platform:comprisesInterfacePart rdf:resource="#theJavaxXmlTransformDomPart"/>
		<platform:comprisesInterfacePart rdf:resource="#theJavaxXmlTransformPart"/>
		<platform:comprisesInterfacePart rdf:resource="#theJavaxXmlParsersPart"/>
		<platform:comprisesInterfacePart rdf:resource="#theJavaxTransactionXaPart"/>
		<platform:comprisesInterfacePart rdf:resource="#theJavaxTransactionPart"/>
		<platform:comprisesInterfacePart rdf:resource="#theJavaxSqlPart"/>
		<platform:comprisesInterfacePart rdf:resource="#theJavaxCryptoSpecPart"/>
		<platform:comprisesInterfacePart rdf:resource="#theJavaxCryptoInterfacesPart"/>
		<platform:comprisesInterfacePart rdf:resource="#theJavaxCryptoPart"/>
		<platform:comprisesInterfacePart rdf:resource="#theJavaxRmiCORBAPart"/>
		<platform:comprisesInterfacePart rdf:resource="#theJavaxRmiPart"/>
		<platform:comprisesInterfacePart rdf:resource="#theJavaxNetSslPart"/>
		<platform:comprisesInterfacePart rdf:resource="#theJavaxNetPart"/>
		<platform:comprisesInterfacePart rdf:resource="#theJavaxNamingSpiPart"/>
		<platform:comprisesInterfacePart rdf:resource="#theJavaxNamingLdapPart"/>
		<platform:comprisesInterfacePart rdf:resource="#theJavaxNamingEventPart"/>
		<platform:comprisesInterfacePart rdf:resource="#theJavaxNamingDirectoryPart"/>
		<platform:comprisesInterfacePart rdf:resource="#theJavaxNamingPart"/>
		<platform:comprisesInterfacePart rdf:resource="#theJavaxSecurityCertPart"/>
		<platform:comprisesInterfacePart rdf:resource="#theJavaxSecurityAuthSpiPart"/>
		<platform:comprisesInterfacePart rdf:resource="#theJavaxSecurityAuthLoginPart"/>
		<platform:comprisesInterfacePart rdf:resource="#theJavaxSecurityAuthKerberosPart"/>
		<platform:comprisesInterfacePart rdf:resource="#theJavaxSecurityAuthCallbackPart"/>
		<platform:comprisesInterfacePart rdf:resource="#theJavaxSecurityAuthX500Part"/>
		<platform:comprisesInterfacePart rdf:resource="#theJavaxSecurityAuthPart"/>
		<platform:comprisesInterfacePart rdf:resource="#theJavaxPrintEventPart"/>
		<platform:comprisesInterfacePart rdf:resource="#theJavaxPrintAttributeStandardPart"/>
		<platform:comprisesInterfacePart rdf:resource="#theJavaxPrintAttributePart"/>
		<platform:comprisesInterfacePart rdf:resource="#theJavaxPrintPart"/>
		<platform:comprisesInterfacePart rdf:resource="#theJavaxSoundMidiSpiPart"/>
		<platform:comprisesInterfacePart rdf:resource="#theJavaxSoundMidiPart"/>
		<platform:comprisesInterfacePart rdf:resource="#theJavaxSoundSampledSpiPart"/>
		<platform:comprisesInterfacePart rdf:resource="#theJavaxSoundSampledPart"/>
		<platform:comprisesInterfacePart rdf:resource="#theJavaxSwingColorchooserPart"/>
		<platform:comprisesInterfacePart rdf:resource="#theJavaxSwingFilechooserPart"/>
		<platform:comprisesInterfacePart rdf:resource="#theJavaxSwingTreePart"/>
		<platform:comprisesInterfacePart rdf:resource="#theJavaxSwingUndoPart"/>
		<platform:comprisesInterfacePart rdf:resource="#theJavaxSwingTablePart"/>
		<platform:comprisesInterfacePart rdf:resource="#theJavaxSwingTextRtfPart"/>
		<platform:comprisesInterfacePart rdf:resource="#theJavaxSwingTextHtmlParserPart"/>
		<platform:comprisesInterfacePart rdf:resource="#theJavaxSwingTextHtmlPart"/>
		<platform:comprisesInterfacePart rdf:resource="#theJavaxSwingTextPart"/>
		<platform:comprisesInterfacePart rdf:resource="#theJavaxSwingBorderPart"/>
		<platform:comprisesInterfacePart rdf:resource="#theJavaxSwingEventPart"/>
		<platform:comprisesInterfacePart rdf:resource="#theJavaxSwingPlafMultiPart"/>
		<platform:comprisesInterfacePart rdf:resource="#theJavaxSwingPlafMetalPart"/>
		<platform:comprisesInterfacePart rdf:resource="#theJavaxSwingPlafBasicPart"/>
		<platform:comprisesInterfacePart rdf:resource="#theJavaxSwingPlafPart"/>
		<platform:comprisesInterfacePart rdf:resource="#theJavaxSwingPart"/>
		<platform:comprisesInterfacePart rdf:resource="#theJavaxAccessibilityPart"/>
		<platform:comprisesInterfacePart rdf:resource="#theJavaxImageioPluginsJpegPart"/>
		<platform:comprisesInterfacePart rdf:resource="#theJavaxImageioEventPart"/>
		<platform:comprisesInterfacePart rdf:resource="#theJavaxImageioStreamPart"/>
		<platform:comprisesInterfacePart rdf:resource="#theJavaxImageioMetadataPart"/>
		<platform:comprisesInterfacePart rdf:resource="#theJavaxImageioSpiPart"/>
		<platform:comprisesInterfacePart rdf:resource="#theJavaxImageioPart"/>
		<platform:comprisesInterfacePart rdf:resource="#theJavaSqlPart"/>
		<platform:comprisesInterfacePart rdf:resource="#theJavaRmiRegistryPart"/>
		<platform:comprisesInterfacePart rdf:resource="#theJavaRmiDgcPart"/>
		<platform:comprisesInterfacePart rdf:resource="#theJavaRmiServerPart"/>
		<platform:comprisesInterfacePart rdf:resource="#theJavaRmiActivationPart"/>
		<platform:comprisesInterfacePart rdf:resource="#theJavaRmiPart"/>
		<platform:comprisesInterfacePart rdf:resource="#theJavaAppletPart"/>
		<platform:comprisesInterfacePart rdf:resource="#theJavaMathPart"/>
		<platform:comprisesInterfacePart rdf:resource="#theJavaTextPart"/>
		<platform:comprisesInterfacePart rdf:resource="#theJavaAwtPrintPart"/>
		<platform:comprisesInterfacePart rdf:resource="#theJavaAwtColorPart"/>
		<platform:comprisesInterfacePart rdf:resource="#theJavaAwtGeomPart"/>
		<platform:comprisesInterfacePart rdf:resource="#theJavaAwtFontPart"/>
		<platform:comprisesInterfacePart rdf:resource="#theJavaAwtImSpiPart"/>
		<platform:comprisesInterfacePart rdf:resource="#theJavaAwtImPart"/>
		<platform:comprisesInterfacePart rdf:resource="#theJavaAwtEventPart"/>
		<platform:comprisesInterfacePart rdf:resource="#theJavaAwtDndPart"/>
		<platform:comprisesInterfacePart rdf:resource="#theJavaAwtDatatransferPart"/>
		<platform:comprisesInterfacePart rdf:resource="#theJavaAwtImageRenderablePart"/>
		<platform:comprisesInterfacePart rdf:resource="#theJavaAwtImagePart"/>
		<platform:comprisesInterfacePart rdf:resource="#theJavaAwtPart"/>
		<platform:comprisesInterfacePart rdf:resource="#theJavaBeansBeancontextPart"/>
		<platform:comprisesInterfacePart rdf:resource="#theJavaBeansPart"/>
		<platform:comprisesInterfacePart rdf:resource="#theJavaNioCharsetSpiPart"/>
		<platform:comprisesInterfacePart rdf:resource="#theJavaNioCharsetPart"/>
		<platform:comprisesInterfacePart rdf:resource="#theJavaNioChannelsSpiPart"/>
		<platform:comprisesInterfacePart rdf:resource="#theJavaNioChannelsPart"/>
		<platform:comprisesInterfacePart rdf:resource="#theJavaNioPart"/>
		<platform:comprisesInterfacePart rdf:resource="#theJavaSecurityInterfacesPart"/>
		<platform:comprisesInterfacePart rdf:resource="#theJavaSecurityAclPart"/>
		<platform:comprisesInterfacePart rdf:resource="#theJavaSecuritySpecPart"/>
		<platform:comprisesInterfacePart rdf:resource="#theJavaSecurityCertPart"/>
		<platform:comprisesInterfacePart rdf:resource="#theJavaSecurityPart"/>
		<platform:comprisesInterfacePart rdf:resource="#theJavaNetPart"/>
		<platform:comprisesInterfacePart rdf:resource="#theJavaUtilRegexPart"/>
		<platform:comprisesInterfacePart rdf:resource="#theJavaUtilPrefsPart"/>
		<platform:comprisesInterfacePart rdf:resource="#theJavaUtilZipPart"/>
		<platform:comprisesInterfacePart rdf:resource="#theJavaUtilJarPart"/>
		<platform:comprisesInterfacePart rdf:resource="#theJavaUtilLoggingPart"/>
		<platform:comprisesInterfacePart rdf:resource="#theJavaUtilPart"/>
		<platform:comprisesInterfacePart rdf:resource="#theJavaIoPart"/>
		<platform:comprisesInterfacePart rdf:resource="#theJavaLangRefPart"/>
		<platform:comprisesInterfacePart rdf:resource="#theJavaLangReflectPart"/>
		<platform:comprisesInterfacePart rdf:resource="#theJavaLangPart"/>
	</J2SE1_4API>
	<owl:Class rdf:about="#J2SE1_4VM">
		<owl:equivalentClass>
			<owl:Restriction>
				<owl:onProperty rdf:resource="&platform;implementsInterface"/>
				<owl:someValuesFrom rdf:resource="#J2SE1_4BytecodeFormat"/>
			</owl:Restriction>
		</owl:equivalentClass>
		<rdfs:subClassOf rdf:resource="&java;JavaVM"/>
		<rdfs:comment xml:lang="en">J2SE 1.4 virtual machine</rdfs:comment>
	</owl:Class>
	<owl:Class rdf:about="#J2SE1_4JRE">
		<owl:equivalentClass>
			<owl:Class >
				<owl:intersectionOf rdf:parseType="Collection">
					<owl:Restriction>
						<owl:onProperty rdf:resource="&platform;providesFeature"/>
						<owl:someValuesFrom rdf:resource="#J2SE1_4ClassLibrary"/>
					</owl:Restriction>
					<owl:Restriction>
						<owl:onProperty rdf:resource="&platform;providesFeature"/>
						<owl:someValuesFrom rdf:resource="#J2SE1_4VM"/>
					</owl:Restriction>
				</owl:intersectionOf>
			</owl:Class>
		</owl:equivalentClass>
		<rdfs:subClassOf rdf:resource="&java;JRE"/>
		<rdfs:comment xml:lang="en">J2SE 1.4 Java Runtime Environment</rdfs:comment>
	</owl:Class>
	<owl:Class rdf:about="#JavaLang">
		<rdfs:subClassOf rdf:resource="&j2me-pp-1_1;JavaLang"/>
		<rdfs:subClassOf rdf:resource="&j2se-1_3;JavaLang"/>
		<rdfs:seeAlso rdf:resource="#JavaNet"/>
		<rdfs:seeAlso rdf:resource="#JavaSecurity"/>
		<rdfs:seeAlso rdf:resource="#JavaUtil"/>
		<rdfs:seeAlso rdf:resource="#JavaIo"/>
		<rdfs:seeAlso rdf:resource="#JavaLangReflect"/>
		<rdfs:comment xml:lang="en">Java API part implementing the java.lang package for J2SE 1.4</rdfs:comment>
	</owl:Class>
	<owl:Class rdf:about="#JavaLangReflect">
		<owl:equivalentClass rdf:resource="&j2me-pp-1_1;JavaLangReflect"/>
		<rdfs:subClassOf rdf:resource="&j2se-1_3;JavaLangReflect"/>
		<rdfs:seeAlso rdf:resource="#JavaSecurity"/>
		<rdfs:seeAlso rdf:resource="#JavaLang"/>
		<rdfs:seeAlso rdf:resource="#JavaIo"/>
		<rdfs:comment xml:lang="en">Java API part implementing the java.lang.reflect package for J2SE 1.4</rdfs:comment>
	</owl:Class>
	<owl:Class rdf:about="#JavaLangRef">
		<owl:equivalentClass rdf:resource="&j2me-pp-1_1;JavaLangRef"/>
		<owl:equivalentClass rdf:resource="&j2se-1_3;JavaLangRef"/>
		<rdfs:subClassOf rdf:resource="&java;JavaAPIPart"/>
		<rdfs:seeAlso rdf:resource="#JavaLang"/>
		<rdfs:comment xml:lang="en">Java API part implementing the java.lang.ref package for J2SE 1.4</rdfs:comment>
	</owl:Class>
	<owl:Class rdf:about="#JavaIo">
		<rdfs:subClassOf rdf:resource="&j2me-pp-1_1;JavaIo"/>
		<rdfs:subClassOf rdf:resource="&j2se-1_3;JavaIo"/>
		<rdfs:seeAlso rdf:resource="#JavaNet"/>
		<rdfs:seeAlso rdf:resource="#JavaNioChannels"/>
		<rdfs:seeAlso rdf:resource="#JavaNioCharset"/>
		<rdfs:seeAlso rdf:resource="#JavaSecurity"/>
		<rdfs:seeAlso rdf:resource="#JavaUtil"/>
		<rdfs:seeAlso rdf:resource="#JavaLang"/>
		<rdfs:comment xml:lang="en">Java API part implementing the java.io package for J2SE 1.4</rdfs:comment>
	</owl:Class>
	<owl:Class rdf:about="#JavaUtil">
		<rdfs:subClassOf rdf:resource="&j2me-pp-1_1;JavaUtil"/>
		<rdfs:subClassOf rdf:resource="&j2se-1_3;JavaUtil"/>
		<rdfs:seeAlso rdf:resource="#JavaSecurity"/>
		<rdfs:seeAlso rdf:resource="#JavaLang"/>
		<rdfs:seeAlso rdf:resource="#JavaIo"/>
		<rdfs:comment xml:lang="en">Java API part implementing the java.util package for J2SE 1.4</rdfs:comment>
	</owl:Class>
	<owl:Class rdf:about="#JavaUtilLogging">
		<rdfs:subClassOf rdf:resource="&java;JavaAPIPart"/>
		<rdfs:seeAlso rdf:resource="#JavaUtil"/>
		<rdfs:seeAlso rdf:resource="#JavaSecurity"/>
		<rdfs:seeAlso rdf:resource="#JavaLang"/>
		<rdfs:seeAlso rdf:resource="#JavaBeans"/>
		<rdfs:seeAlso rdf:resource="#JavaIo"/>
		<rdfs:comment xml:lang="en">Java API part implementing the java.util.logging package for J2SE 1.4</rdfs:comment>
	</owl:Class>
	<owl:Class rdf:about="#JavaUtilJar">
		<owl:equivalentClass rdf:resource="&j2me-pp-1_1;JavaUtilJar"/>
		<rdfs:subClassOf rdf:resource="&j2se-1_3;JavaUtilJar"/>
		<rdfs:seeAlso rdf:resource="#JavaUtil"/>
		<rdfs:seeAlso rdf:resource="#JavaLang"/>
		<rdfs:seeAlso rdf:resource="#JavaIo"/>
		<rdfs:seeAlso rdf:resource="#JavaUtilZip"/>
		<rdfs:comment xml:lang="en">Java API part implementing the java.util.jar package for J2SE 1.4</rdfs:comment>
	</owl:Class>
	<owl:Class rdf:about="#JavaUtilZip">
		<owl:equivalentClass rdf:resource="&j2me-pp-1_1;JavaUtilZip"/>
		<rdfs:subClassOf rdf:resource="&j2se-1_3;JavaUtilZip"/>
		<rdfs:seeAlso rdf:resource="#JavaUtil"/>
		<rdfs:seeAlso rdf:resource="#JavaLang"/>
		<rdfs:seeAlso rdf:resource="#JavaIo"/>
		<rdfs:comment xml:lang="en">Java API part implementing the java.util.zip package for J2SE 1.4</rdfs:comment>
	</owl:Class>
	<owl:Class rdf:about="#JavaUtilPrefs">
		<rdfs:subClassOf rdf:resource="&java;JavaAPIPart"/>
		<rdfs:seeAlso rdf:resource="#JavaUtil"/>
		<rdfs:seeAlso rdf:resource="#JavaLang"/>
		<rdfs:seeAlso rdf:resource="#JavaIo"/>
		<rdfs:comment xml:lang="en">Java API part implementing the java.util.prefs package for J2SE 1.4</rdfs:comment>
	</owl:Class>
	<owl:Class rdf:about="#JavaUtilRegex">
		<rdfs:subClassOf rdf:resource="&java;JavaAPIPart"/>
		<rdfs:seeAlso rdf:resource="#JavaLang"/>
		<rdfs:seeAlso rdf:resource="#JavaIo"/>
		<rdfs:comment xml:lang="en">Java API part implementing the java.util.regex package for J2SE 1.4</rdfs:comment>
	</owl:Class>
	<owl:Class rdf:about="#JavaNet">
		<rdfs:subClassOf rdf:resource="&j2me-pp-1_1;JavaNet"/>
		<rdfs:subClassOf rdf:resource="&j2se-1_3;JavaNet"/>
		<rdfs:seeAlso rdf:resource="#JavaUtil"/>
		<rdfs:seeAlso rdf:resource="#JavaSecurity"/>
		<rdfs:seeAlso rdf:resource="#JavaLang"/>
		<rdfs:seeAlso rdf:resource="#JavaIo"/>
		<rdfs:seeAlso rdf:resource="#JavaNioChannels"/>
		<rdfs:seeAlso rdf:resource="#JavaUtilJar"/>
		<rdfs:comment xml:lang="en">Java API part implementing the java.net package for J2SE 1.4</rdfs:comment>
	</owl:Class>
	<owl:Class rdf:about="#JavaSecurity">
		<rdfs:subClassOf rdf:resource="&j2me-pp-1_1;JavaSecurity"/>
		<rdfs:subClassOf rdf:resource="&j2se-1_3;JavaSecurity"/>
		<rdfs:seeAlso rdf:resource="#JavaSecurityCert"/>
		<rdfs:seeAlso rdf:resource="#JavaSecuritySpec"/>
		<rdfs:seeAlso rdf:resource="#JavaUtil"/>
		<rdfs:seeAlso rdf:resource="#JavaLang"/>
		<rdfs:seeAlso rdf:resource="#JavaIo"/>
		<rdfs:seeAlso rdf:resource="#JavaNet"/>
		<rdfs:comment xml:lang="en">Java API part implementing the java.security package for J2SE 1.4</rdfs:comment>
	</owl:Class>
	<owl:Class rdf:about="#JavaSecurityCert">
		<rdfs:subClassOf rdf:resource="&j2me-pp-1_1;JavaSecurityCert"/>
		<rdfs:subClassOf rdf:resource="&j2se-1_3;JavaSecurityCert"/>
		<rdfs:seeAlso rdf:resource="#JavaMath"/>
		<rdfs:seeAlso rdf:resource="#JavaUtil"/>
		<rdfs:seeAlso rdf:resource="#JavaSecurity"/>
		<rdfs:seeAlso rdf:resource="#JavaLang"/>
		<rdfs:seeAlso rdf:resource="#JavaxSecurityAuthX500"/>
		<rdfs:seeAlso rdf:resource="#JavaIo"/>
		<rdfs:comment xml:lang="en">Java API part implementing the java.security.cert package for J2SE 1.4</rdfs:comment>
	</owl:Class>
	<owl:Class rdf:about="#JavaSecuritySpec">
		<rdfs:subClassOf rdf:resource="&j2me-pp-1_1;JavaSecuritySpec"/>
		<rdfs:subClassOf rdf:resource="&j2se-1_3;JavaSecuritySpec"/>
		<rdfs:seeAlso rdf:resource="#JavaSecurity"/>
		<rdfs:seeAlso rdf:resource="#JavaLang"/>
		<rdfs:seeAlso rdf:resource="#JavaSecurityInterfaces"/>
		<rdfs:seeAlso rdf:resource="#JavaMath"/>
		<rdfs:comment xml:lang="en">Java API part implementing the java.security.spec package for J2SE 1.4</rdfs:comment>
	</owl:Class>
	<owl:Class rdf:about="#JavaSecurityAcl">
		<owl:equivalentClass rdf:resource="&j2me-pp-1_1;JavaSecurityAcl"/>
		<rdfs:subClassOf rdf:resource="&j2se-1_3;JavaSecurityAcl"/>
		<rdfs:seeAlso rdf:resource="#JavaSecurity"/>
		<rdfs:seeAlso rdf:resource="#JavaUtil"/>
		<rdfs:seeAlso rdf:resource="#JavaLang"/>
		<rdfs:comment xml:lang="en">Java API part implementing the java.security.acl package for J2SE 1.4</rdfs:comment>
	</owl:Class>
	<owl:Class rdf:about="#JavaSecurityInterfaces">
		<rdfs:subClassOf rdf:resource="&j2me-pp-1_1;JavaSecurityInterfaces"/>
		<rdfs:subClassOf rdf:resource="&j2se-1_3;JavaSecurityInterfaces"/>
		<rdfs:seeAlso rdf:resource="#JavaSecurity"/>
		<rdfs:seeAlso rdf:resource="#JavaMath"/>
		<rdfs:comment xml:lang="en">Java API part implementing the java.security.interfaces package for J2SE 1.4</rdfs:comment>
	</owl:Class>
	<owl:Class rdf:about="#JavaNio">
		<rdfs:subClassOf rdf:resource="&java;JavaAPIPart"/>
		<rdfs:seeAlso rdf:resource="#JavaLang"/>
		<rdfs:comment xml:lang="en">Java API part implementing the java.nio package for J2SE 1.4</rdfs:comment>
	</owl:Class>
	<owl:Class rdf:about="#JavaNioChannels">
		<rdfs:subClassOf rdf:resource="&java;JavaAPIPart"/>
		<rdfs:seeAlso rdf:resource="#JavaNet"/>
		<rdfs:seeAlso rdf:resource="#JavaNioCharset"/>
		<rdfs:seeAlso rdf:resource="#JavaUtil"/>
		<rdfs:seeAlso rdf:resource="#JavaLang"/>
		<rdfs:seeAlso rdf:resource="#JavaIo"/>
		<rdfs:seeAlso rdf:resource="#JavaNio"/>
		<rdfs:seeAlso rdf:resource="#JavaNioChannelsSpi"/>
		<rdfs:comment xml:lang="en">Java API part implementing the java.nio.channels package for J2SE 1.4</rdfs:comment>
	</owl:Class>
	<owl:Class rdf:about="#JavaNioChannelsSpi">
		<rdfs:subClassOf rdf:resource="&java;JavaAPIPart"/>
		<rdfs:seeAlso rdf:resource="#JavaUtil"/>
		<rdfs:seeAlso rdf:resource="#JavaLang"/>
		<rdfs:seeAlso rdf:resource="#JavaNioChannels"/>
		<rdfs:comment xml:lang="en">Java API part implementing the java.nio.channels.spi package for J2SE 1.4</rdfs:comment>
	</owl:Class>
	<owl:Class rdf:about="#JavaNioCharset">
		<rdfs:subClassOf rdf:resource="&java;JavaAPIPart"/>
		<rdfs:seeAlso rdf:resource="#JavaUtil"/>
		<rdfs:seeAlso rdf:resource="#JavaLang"/>
		<rdfs:seeAlso rdf:resource="#JavaIo"/>
		<rdfs:seeAlso rdf:resource="#JavaNio"/>
		<rdfs:comment xml:lang="en">Java API part implementing the java.nio.charset package for J2SE 1.4</rdfs:comment>
	</owl:Class>
	<owl:Class rdf:about="#JavaNioCharsetSpi">
		<rdfs:subClassOf rdf:resource="&java;JavaAPIPart"/>
		<rdfs:seeAlso rdf:resource="#JavaNioCharset"/>
		<rdfs:seeAlso rdf:resource="#JavaUtil"/>
		<rdfs:seeAlso rdf:resource="#JavaLang"/>
		<rdfs:comment xml:lang="en">Java API part implementing the java.nio.charset.spi package for J2SE 1.4</rdfs:comment>
	</owl:Class>
	<owl:Class rdf:about="#JavaBeans">
		<rdfs:subClassOf rdf:resource="&j2me-pp-1_1;JavaBeans"/>
		<rdfs:subClassOf rdf:resource="&j2se-1_3;JavaBeans"/>
		<rdfs:seeAlso rdf:resource="#JavaAwt"/>
		<rdfs:seeAlso rdf:resource="#JavaBeansBeancontext"/>
		<rdfs:seeAlso rdf:resource="#JavaApplet"/>
		<rdfs:seeAlso rdf:resource="#JavaUtil"/>
		<rdfs:seeAlso rdf:resource="#JavaLang"/>
		<rdfs:seeAlso rdf:resource="#JavaIo"/>
		<rdfs:seeAlso rdf:resource="#JavaLangReflect"/>
		<rdfs:comment xml:lang="en">Java API part implementing the java.beans package for J2SE 1.4</rdfs:comment>
	</owl:Class>
	<owl:Class rdf:about="#JavaBeansBeancontext">
		<owl:equivalentClass rdf:resource="&j2se-1_3;JavaBeansBeancontext"/>
		<rdfs:subClassOf rdf:resource="&java;JavaAPIPart"/>
		<rdfs:seeAlso rdf:resource="#JavaAwt"/>
		<rdfs:seeAlso rdf:resource="#JavaUtil"/>
		<rdfs:seeAlso rdf:resource="#JavaLang"/>
		<rdfs:seeAlso rdf:resource="#JavaIo"/>
		<rdfs:seeAlso rdf:resource="#JavaNet"/>
		<rdfs:seeAlso rdf:resource="#JavaBeans"/>
		<rdfs:comment xml:lang="en">Java API part implementing the java.beans.beancontext package for J2SE 1.4</rdfs:comment>
	</owl:Class>
	<owl:Class rdf:about="#JavaAwt">
		<rdfs:subClassOf rdf:resource="&j2me-pp-1_1;JavaAwt"/>
		<rdfs:subClassOf rdf:resource="&j2se-1_3;JavaAwt"/>
		<rdfs:seeAlso rdf:resource="#JavaLang"/>
		<rdfs:seeAlso rdf:resource="#JavaNet"/>
		<rdfs:seeAlso rdf:resource="#JavaAwtDnd"/>
		<rdfs:seeAlso rdf:resource="#JavaBeans"/>
		<rdfs:seeAlso rdf:resource="#JavaAwtEvent"/>
		<rdfs:seeAlso rdf:resource="#JavaxSwingText"/>
		<rdfs:seeAlso rdf:resource="#JavaSecurity"/>
		<rdfs:seeAlso rdf:resource="#JavaUtil"/>
		<rdfs:seeAlso rdf:resource="#JavaIo"/>
		<rdfs:seeAlso rdf:resource="#JavaText"/>
		<rdfs:seeAlso rdf:resource="#JavaAwtGeom"/>
		<rdfs:seeAlso rdf:resource="#JavaAwtIm"/>
		<rdfs:seeAlso rdf:resource="#JavaAwtDatatransfer"/>
		<rdfs:seeAlso rdf:resource="#JavaxAccessibility"/>
		<rdfs:seeAlso rdf:resource="#JavaAwtFont"/>
		<rdfs:seeAlso rdf:resource="#JavaAwtImageRenderable"/>
		<rdfs:seeAlso rdf:resource="#JavaAwtColor"/>
		<rdfs:seeAlso rdf:resource="#JavaAwtImage"/>
		<rdfs:comment xml:lang="en">Java API part implementing the java.awt package for J2SE 1.4</rdfs:comment>
	</owl:Class>
	<owl:Class rdf:about="#JavaAwtImage">
		<rdfs:subClassOf rdf:resource="&j2me-pp-1_1;JavaAwtImage"/>
		<rdfs:subClassOf rdf:resource="&j2se-1_3;JavaAwtImage"/>
		<rdfs:seeAlso rdf:resource="#JavaAwt"/>
		<rdfs:seeAlso rdf:resource="#JavaMath"/>
		<rdfs:seeAlso rdf:resource="#JavaAwtGeom"/>
		<rdfs:seeAlso rdf:resource="#JavaUtil"/>
		<rdfs:seeAlso rdf:resource="#JavaLang"/>
		<rdfs:seeAlso rdf:resource="#JavaAwtColor"/>
		<rdfs:comment xml:lang="en">Java API part implementing the java.awt.image package for J2SE 1.4</rdfs:comment>
	</owl:Class>
	<owl:Class rdf:about="#JavaAwtImageRenderable">
		<owl:equivalentClass rdf:resource="&j2se-1_3;JavaAwtImageRenderable"/>
		<rdfs:subClassOf rdf:resource="&java;JavaAPIPart"/>
		<rdfs:seeAlso rdf:resource="#JavaAwt"/>
		<rdfs:seeAlso rdf:resource="#JavaAwtGeom"/>
		<rdfs:seeAlso rdf:resource="#JavaUtil"/>
		<rdfs:seeAlso rdf:resource="#JavaLang"/>
		<rdfs:seeAlso rdf:resource="#JavaIo"/>
		<rdfs:seeAlso rdf:resource="#JavaAwtImage"/>
		<rdfs:comment xml:lang="en">Java API part implementing the java.awt.image.renderable package for J2SE 1.4</rdfs:comment>
	</owl:Class>
	<owl:Class rdf:about="#JavaAwtDatatransfer">
		<rdfs:subClassOf rdf:resource="&j2me-pp-1_1;JavaAwtDatatransfer"/>
		<rdfs:subClassOf rdf:resource="&j2se-1_3;JavaAwtDatatransfer"/>
		<rdfs:seeAlso rdf:resource="#JavaUtil"/>
		<rdfs:seeAlso rdf:resource="#JavaLang"/>
		<rdfs:seeAlso rdf:resource="#JavaIo"/>
		<rdfs:comment xml:lang="en">Java API part implementing the java.awt.datatransfer package for J2SE 1.4</rdfs:comment>
	</owl:Class>
	<owl:Class rdf:about="#JavaAwtDnd">
		<rdfs:subClassOf rdf:resource="&j2se-1_3;JavaAwtDnd"/>
		<rdfs:seeAlso rdf:resource="#JavaAwtDatatransfer"/>
		<rdfs:seeAlso rdf:resource="#JavaAwt"/>
		<rdfs:seeAlso rdf:resource="#JavaUtil"/>
		<rdfs:seeAlso rdf:resource="#JavaLang"/>
		<rdfs:seeAlso rdf:resource="#JavaIo"/>
		<rdfs:seeAlso rdf:resource="#JavaAwtEvent"/>
		<rdfs:comment xml:lang="en">Java API part implementing the java.awt.dnd package for J2SE 1.4</rdfs:comment>
	</owl:Class>
	<owl:Class rdf:about="#JavaAwtEvent">
		<rdfs:subClassOf rdf:resource="&j2me-pp-1_1;JavaAwtEvent"/>
		<rdfs:subClassOf rdf:resource="&j2se-1_3;JavaAwtEvent"/>
		<rdfs:seeAlso rdf:resource="#JavaAwtFont"/>
		<rdfs:seeAlso rdf:resource="#JavaText"/>
		<rdfs:seeAlso rdf:resource="#JavaAwt"/>
		<rdfs:seeAlso rdf:resource="#JavaUtil"/>
		<rdfs:seeAlso rdf:resource="#JavaLang"/>
		<rdfs:comment xml:lang="en">Java API part implementing the java.awt.event package for J2SE 1.4</rdfs:comment>
	</owl:Class>
	<owl:Class rdf:about="#JavaAwtIm">
		<owl:equivalentClass rdf:resource="&j2se-1_3;JavaAwtIm"/>
		<rdfs:subClassOf rdf:resource="&j2me-pp-1_1;JavaAwtIm"/>
		<rdfs:seeAlso rdf:resource="#JavaUtil"/>
		<rdfs:seeAlso rdf:resource="#JavaAwtFont"/>
		<rdfs:seeAlso rdf:resource="#JavaLang"/>
		<rdfs:seeAlso rdf:resource="#JavaText"/>
		<rdfs:seeAlso rdf:resource="#JavaAwt"/>
		<rdfs:comment xml:lang="en">Java API part implementing the java.awt.im package for J2SE 1.4</rdfs:comment>
	</owl:Class>
	<owl:Class rdf:about="#JavaAwtImSpi">
		<rdfs:subClassOf rdf:resource="&j2se-1_3;JavaAwtImSpi"/>
		<rdfs:seeAlso rdf:resource="#JavaAwtIm"/>
		<rdfs:seeAlso rdf:resource="#JavaUtil"/>
		<rdfs:seeAlso rdf:resource="#JavaAwtFont"/>
		<rdfs:seeAlso rdf:resource="#JavaLang"/>
		<rdfs:seeAlso rdf:resource="#JavaText"/>
		<rdfs:seeAlso rdf:resource="#JavaAwt"/>
		<rdfs:seeAlso rdf:resource="#JavaxSwing"/>
		<rdfs:comment xml:lang="en">Java API part implementing the java.awt.im.spi package for J2SE 1.4</rdfs:comment>
	</owl:Class>
	<owl:Class rdf:about="#JavaAwtFont">
		<rdfs:subClassOf rdf:resource="&j2me-pp-1_1;JavaAwtFont"/>
		<rdfs:subClassOf rdf:resource="&j2se-1_3;JavaAwtFont"/>
		<rdfs:seeAlso rdf:resource="#JavaText"/>
		<rdfs:seeAlso rdf:resource="#JavaAwt"/>
		<rdfs:seeAlso rdf:resource="#JavaAwtGeom"/>
		<rdfs:seeAlso rdf:resource="#JavaUtil"/>
		<rdfs:seeAlso rdf:resource="#JavaLang"/>
		<rdfs:seeAlso rdf:resource="#JavaIo"/>
		<rdfs:comment xml:lang="en">Java API part implementing the java.awt.font package for J2SE 1.4</rdfs:comment>
	</owl:Class>
	<owl:Class rdf:about="#JavaAwtGeom">
		<rdfs:subClassOf rdf:resource="&j2se-1_3;JavaAwtGeom"/>
		<rdfs:seeAlso rdf:resource="#JavaLang"/>
		<rdfs:seeAlso rdf:resource="#JavaAwt"/>
		<rdfs:seeAlso rdf:resource="#JavaIo"/>
		<rdfs:comment xml:lang="en">Java API part implementing the java.awt.geom package for J2SE 1.4</rdfs:comment>
	</owl:Class>
	<owl:Class rdf:about="#JavaAwtColor">
		<rdfs:subClassOf rdf:resource="&j2me-pp-1_1;JavaAwtColor"/>
		<rdfs:subClassOf rdf:resource="&j2se-1_3;JavaAwtColor"/>
		<rdfs:seeAlso rdf:resource="#JavaLang"/>
		<rdfs:seeAlso rdf:resource="#JavaIo"/>
		<rdfs:comment xml:lang="en">Java API part implementing the java.awt.color package for J2SE 1.4</rdfs:comment>
	</owl:Class>
	<owl:Class rdf:about="#JavaAwtPrint">
		<rdfs:subClassOf rdf:resource="&j2se-1_3;JavaAwtPrint"/>
		<rdfs:seeAlso rdf:resource="#JavaLang"/>
		<rdfs:seeAlso rdf:resource="#JavaxPrintAttribute"/>
		<rdfs:seeAlso rdf:resource="#JavaAwt"/>
		<rdfs:seeAlso rdf:resource="#JavaIo"/>
		<rdfs:seeAlso rdf:resource="#JavaxPrint"/>
		<rdfs:comment xml:lang="en">Java API part implementing the java.awt.print package for J2SE 1.4</rdfs:comment>
	</owl:Class>
	<owl:Class rdf:about="#JavaText">
		<rdfs:subClassOf rdf:resource="&j2se-1_3;JavaText"/>
		<rdfs:seeAlso rdf:resource="#JavaUtil"/>
		<rdfs:seeAlso rdf:resource="#JavaLang"/>
		<rdfs:seeAlso rdf:resource="#JavaIo"/>
		<rdfs:comment xml:lang="en">Java API part implementing the java.text package for J2SE 1.4</rdfs:comment>
	</owl:Class>
	<owl:Class rdf:about="#JavaMath">
		<rdfs:subClassOf rdf:resource="&j2me-pp-1_1;JavaMath"/>
		<rdfs:subClassOf rdf:resource="&j2se-1_3;JavaMath"/>
		<rdfs:seeAlso rdf:resource="#JavaUtil"/>
		<rdfs:seeAlso rdf:resource="#JavaLang"/>
		<rdfs:comment xml:lang="en">Java API part implementing the java.math package for J2SE 1.4</rdfs:comment>
	</owl:Class>
	<owl:Class rdf:about="#JavaApplet">
		<rdfs:subClassOf rdf:resource="&j2me-pp-1_1;JavaApplet"/>
		<rdfs:subClassOf rdf:resource="&j2se-1_3;JavaApplet"/>
		<rdfs:seeAlso rdf:resource="#JavaNet"/>
		<rdfs:seeAlso rdf:resource="#JavaxAccessibility"/>
		<rdfs:seeAlso rdf:resource="#JavaAwt"/>
		<rdfs:seeAlso rdf:resource="#JavaUtil"/>
		<rdfs:seeAlso rdf:resource="#JavaLang"/>
		<rdfs:seeAlso rdf:resource="#JavaIo"/>
		<rdfs:comment xml:lang="en">Java API part implementing the java.applet package for J2SE 1.4</rdfs:comment>
	</owl:Class>
	<owl:Class rdf:about="#JavaRmi">
		<rdfs:subClassOf rdf:resource="&j2me-pp-1_1;JavaRmi"/>
		<rdfs:subClassOf rdf:resource="&j2se-1_3;JavaRmi"/>
		<rdfs:seeAlso rdf:resource="#JavaLang"/>
		<rdfs:seeAlso rdf:resource="#JavaIo"/>
		<rdfs:comment xml:lang="en">Java API part implementing the java.rmi package for J2SE 1.4</rdfs:comment>
	</owl:Class>
	<owl:Class rdf:about="#JavaRmiActivation">
		<rdfs:subClassOf rdf:resource="&j2se-1_3;JavaRmiActivation"/>
		<rdfs:seeAlso rdf:resource="#JavaRmiServer"/>
		<rdfs:seeAlso rdf:resource="#JavaUtil"/>
		<rdfs:seeAlso rdf:resource="#JavaLang"/>
		<rdfs:seeAlso rdf:resource="#JavaIo"/>
		<rdfs:seeAlso rdf:resource="#JavaRmi"/>
		<rdfs:comment xml:lang="en">Java API part implementing the java.rmi.activation package for J2SE 1.4</rdfs:comment>
	</owl:Class>
	<owl:Class rdf:about="#JavaRmiServer">
		<rdfs:subClassOf rdf:resource="&j2se-1_3;JavaRmiServer"/>
		<rdfs:seeAlso rdf:resource="#JavaNet"/>
		<rdfs:seeAlso rdf:resource="#JavaLang"/>
		<rdfs:seeAlso rdf:resource="#JavaIo"/>
		<rdfs:seeAlso rdf:resource="#JavaLangReflect"/>
		<rdfs:seeAlso rdf:resource="#JavaRmi"/>
		<rdfs:comment xml:lang="en">Java API part implementing the java.rmi.server package for J2SE 1.4</rdfs:comment>
	</owl:Class>
	<owl:Class rdf:about="#JavaRmiDgc">
		<owl:equivalentClass rdf:resource="&j2se-1_3;JavaRmiDgc"/>
		<rdfs:subClassOf rdf:resource="&java;JavaAPIPart"/>
		<rdfs:seeAlso rdf:resource="#JavaLang"/>
		<rdfs:seeAlso rdf:resource="#JavaIo"/>
		<rdfs:seeAlso rdf:resource="#JavaRmi"/>
		<rdfs:comment xml:lang="en">Java API part implementing the java.rmi.dgc package for J2SE 1.4</rdfs:comment>
	</owl:Class>
	<owl:Class rdf:about="#JavaRmiRegistry">
		<owl:equivalentClass rdf:resource="&j2se-1_3;JavaRmiRegistry"/>
		<rdfs:subClassOf rdf:resource="&j2me-pp-1_1;JavaRmiRegistry"/>
		<rdfs:seeAlso rdf:resource="#JavaRmiServer"/>
		<rdfs:seeAlso rdf:resource="#JavaLang"/>
		<rdfs:seeAlso rdf:resource="#JavaRmi"/>
		<rdfs:comment xml:lang="en">Java API part implementing the java.rmi.registry package for J2SE 1.4</rdfs:comment>
	</owl:Class>
	<owl:Class rdf:about="#JavaSql">
		<rdfs:subClassOf rdf:resource="&j2se-1_3;JavaSql"/>
		<rdfs:seeAlso rdf:resource="#JavaNet"/>
		<rdfs:seeAlso rdf:resource="#JavaMath"/>
		<rdfs:seeAlso rdf:resource="#JavaSecurity"/>
		<rdfs:seeAlso rdf:resource="#JavaUtil"/>
		<rdfs:seeAlso rdf:resource="#JavaLang"/>
		<rdfs:seeAlso rdf:resource="#JavaIo"/>
		<rdfs:comment xml:lang="en">Java API part implementing the java.sql package for J2SE 1.4</rdfs:comment>
	</owl:Class>
	<owl:Class rdf:about="#JavaxImageio">
		<rdfs:subClassOf rdf:resource="&java;JavaAPIPart"/>
		<rdfs:seeAlso rdf:resource="#JavaAwt"/>
		<rdfs:seeAlso rdf:resource="#JavaUtil"/>
		<rdfs:seeAlso rdf:resource="#JavaLang"/>
		<rdfs:seeAlso rdf:resource="#JavaIo"/>
		<rdfs:seeAlso rdf:resource="#JavaxImageioMetadata"/>
		<rdfs:seeAlso rdf:resource="#JavaNet"/>
		<rdfs:seeAlso rdf:resource="#JavaxImageioEvent"/>
		<rdfs:seeAlso rdf:resource="#JavaxImageioStream"/>
		<rdfs:seeAlso rdf:resource="#JavaxImageioSpi"/>
		<rdfs:seeAlso rdf:resource="#JavaAwtColor"/>
		<rdfs:seeAlso rdf:resource="#JavaAwtImage"/>
		<rdfs:comment xml:lang="en">Java API part implementing the javax.imageio package for J2SE 1.4</rdfs:comment>
	</owl:Class>
	<owl:Class rdf:about="#JavaxImageioSpi">
		<rdfs:subClassOf rdf:resource="&java;JavaAPIPart"/>
		<rdfs:seeAlso rdf:resource="#JavaxImageioStream"/>
		<rdfs:seeAlso rdf:resource="#JavaxImageio"/>
		<rdfs:seeAlso rdf:resource="#JavaUtil"/>
		<rdfs:seeAlso rdf:resource="#JavaLang"/>
		<rdfs:seeAlso rdf:resource="#JavaIo"/>
		<rdfs:seeAlso rdf:resource="#JavaAwtImage"/>
		<rdfs:seeAlso rdf:resource="#JavaxImageioMetadata"/>
		<rdfs:comment xml:lang="en">Java API part implementing the javax.imageio.spi package for J2SE 1.4</rdfs:comment>
	</owl:Class>
	<owl:Class rdf:about="#JavaxImageioMetadata">
		<rdfs:subClassOf rdf:resource="&java;JavaAPIPart"/>
		<rdfs:seeAlso rdf:resource="#JavaxImageio"/>
		<rdfs:seeAlso rdf:resource="#OrgW3cDom"/>
		<rdfs:seeAlso rdf:resource="#JavaUtil"/>
		<rdfs:seeAlso rdf:resource="#JavaLang"/>
		<rdfs:comment xml:lang="en">Java API part implementing the javax.imageio.metadata package for J2SE 1.4</rdfs:comment>
	</owl:Class>
	<owl:Class rdf:about="#JavaxImageioStream">
		<rdfs:subClassOf rdf:resource="&java;JavaAPIPart"/>
		<rdfs:seeAlso rdf:resource="#JavaLang"/>
		<rdfs:seeAlso rdf:resource="#JavaIo"/>
		<rdfs:seeAlso rdf:resource="#JavaNio"/>
		<rdfs:comment xml:lang="en">Java API part implementing the javax.imageio.stream package for J2SE 1.4</rdfs:comment>
	</owl:Class>
	<owl:Class rdf:about="#JavaxImageioEvent">
		<rdfs:subClassOf rdf:resource="&java;JavaAPIPart"/>
		<rdfs:seeAlso rdf:resource="#JavaUtil"/>
		<rdfs:seeAlso rdf:resource="#JavaLang"/>
		<rdfs:seeAlso rdf:resource="#JavaxImageio"/>
		<rdfs:seeAlso rdf:resource="#JavaAwtImage"/>
		<rdfs:comment xml:lang="en">Java API part implementing the javax.imageio.event package for J2SE 1.4</rdfs:comment>
	</owl:Class>
	<owl:Class rdf:about="#JavaxImageioPluginsJpeg">
		<rdfs:subClassOf rdf:resource="&java;JavaAPIPart"/>
		<rdfs:seeAlso rdf:resource="#JavaUtil"/>
		<rdfs:seeAlso rdf:resource="#JavaLang"/>
		<rdfs:seeAlso rdf:resource="#JavaxImageio"/>
		<rdfs:comment xml:lang="en">Java API part implementing the javax.imageio.plugins.jpeg package for J2SE 1.4</rdfs:comment>
	</owl:Class>
	<owl:Class rdf:about="#JavaxAccessibility">
		<rdfs:subClassOf rdf:resource="&j2se-1_3;JavaxAccessibility"/>
		<rdfs:seeAlso rdf:resource="#JavaBeans"/>
		<rdfs:seeAlso rdf:resource="#JavaAwt"/>
		<rdfs:seeAlso rdf:resource="#JavaxSwingText"/>
		<rdfs:seeAlso rdf:resource="#JavaUtil"/>
		<rdfs:seeAlso rdf:resource="#JavaAwtEvent"/>
		<rdfs:seeAlso rdf:resource="#JavaLang"/>
		<rdfs:comment xml:lang="en">Java API part implementing the javax.accessibility package for J2SE 1.4</rdfs:comment>
	</owl:Class>
	<owl:Class rdf:about="#JavaxSwing">
		<rdfs:subClassOf rdf:resource="&java;JavaAPIPart"/>
		<rdfs:seeAlso rdf:resource="#JavaAwt"/>
		<rdfs:seeAlso rdf:resource="#JavaNet"/>
		<rdfs:seeAlso rdf:resource="#JavaAwtEvent"/>
		<rdfs:seeAlso rdf:resource="#JavaUtil"/>
		<rdfs:seeAlso rdf:resource="#JavaxSwingPlaf"/>
		<rdfs:seeAlso rdf:resource="#JavaIo"/>
		<rdfs:seeAlso rdf:resource="#JavaAwtDatatransfer"/>
		<rdfs:seeAlso rdf:resource="#JavaxSwingEvent"/>
		<rdfs:seeAlso rdf:resource="#JavaxAccessibility"/>
		<rdfs:seeAlso rdf:resource="#JavaxSwingFilechooser"/>
		<rdfs:seeAlso rdf:resource="#JavaApplet"/>
		<rdfs:seeAlso rdf:resource="#JavaxSwingTable"/>
		<rdfs:seeAlso rdf:resource="#JavaLang"/>
		<rdfs:seeAlso rdf:resource="#JavaxSwingColorchooser"/>
		<rdfs:seeAlso rdf:resource="#JavaBeans"/>
		<rdfs:seeAlso rdf:resource="#JavaxSwingText"/>
		<rdfs:seeAlso rdf:resource="#JavaText"/>
		<rdfs:seeAlso rdf:resource="#JavaxSwingBorder"/>
		<rdfs:seeAlso rdf:resource="#JavaxSwingTree"/>
		<rdfs:seeAlso rdf:resource="#JavaAwtImage"/>
		<rdfs:comment xml:lang="en">Java API part implementing the javax.swing package for J2SE 1.4</rdfs:comment>
	</owl:Class>
	<owl:Class rdf:about="#JavaxSwingPlaf">
		<rdfs:subClassOf rdf:resource="&j2se-1_3;JavaxSwingPlaf"/>
		<rdfs:seeAlso rdf:resource="#JavaAwt"/>
		<rdfs:seeAlso rdf:resource="#JavaxSwingText"/>
		<rdfs:seeAlso rdf:resource="#JavaLang"/>
		<rdfs:seeAlso rdf:resource="#JavaIo"/>
		<rdfs:seeAlso rdf:resource="#JavaxSwingBorder"/>
		<rdfs:seeAlso rdf:resource="#JavaxAccessibility"/>
		<rdfs:seeAlso rdf:resource="#JavaxSwing"/>
		<rdfs:seeAlso rdf:resource="#JavaAwtEvent"/>
		<rdfs:seeAlso rdf:resource="#JavaxSwingTree"/>
		<rdfs:seeAlso rdf:resource="#JavaxSwingFilechooser"/>
		<rdfs:comment xml:lang="en">Java API part implementing the javax.swing.plaf package for J2SE 1.4</rdfs:comment>
	</owl:Class>
	<owl:Class rdf:about="#JavaxSwingPlafBasic">
		<rdfs:subClassOf rdf:resource="&j2se-1_3;JavaxSwingPlafBasic"/>
		<rdfs:seeAlso rdf:resource="#JavaAwt"/>
		<rdfs:seeAlso rdf:resource="#JavaxSwingTable"/>
		<rdfs:seeAlso rdf:resource="#JavaLang"/>
		<rdfs:seeAlso rdf:resource="#JavaBeans"/>
		<rdfs:seeAlso rdf:resource="#JavaAwtEvent"/>
		<rdfs:seeAlso rdf:resource="#JavaxSwingText"/>
		<rdfs:seeAlso rdf:resource="#JavaUtil"/>
		<rdfs:seeAlso rdf:resource="#JavaxSwingPlaf"/>
		<rdfs:seeAlso rdf:resource="#JavaIo"/>
		<rdfs:seeAlso rdf:resource="#JavaxSwingEvent"/>
		<rdfs:seeAlso rdf:resource="#JavaxSwingBorder"/>
		<rdfs:seeAlso rdf:resource="#JavaxAccessibility"/>
		<rdfs:seeAlso rdf:resource="#JavaxSwing"/>
		<rdfs:seeAlso rdf:resource="#JavaxSwingTree"/>
		<rdfs:seeAlso rdf:resource="#JavaxSwingFilechooser"/>
		<rdfs:comment xml:lang="en">Java API part implementing the javax.swing.plaf.basic package for J2SE 1.4</rdfs:comment>
	</owl:Class>
	<owl:Class rdf:about="#JavaxSwingPlafMetal">
		<rdfs:subClassOf rdf:resource="&j2se-1_3;JavaxSwingPlafMetal"/>
		<rdfs:seeAlso rdf:resource="#JavaAwt"/>
		<rdfs:seeAlso rdf:resource="#JavaLang"/>
		<rdfs:seeAlso rdf:resource="#JavaxSwingPlafBasic"/>
		<rdfs:seeAlso rdf:resource="#JavaxSwingEvent"/>
		<rdfs:seeAlso rdf:resource="#JavaxSwingBorder"/>
		<rdfs:seeAlso rdf:resource="#JavaBeans"/>
		<rdfs:seeAlso rdf:resource="#JavaxSwing"/>
		<rdfs:seeAlso rdf:resource="#JavaAwtEvent"/>
		<rdfs:seeAlso rdf:resource="#JavaxSwingTree"/>
		<rdfs:seeAlso rdf:resource="#JavaxSwingPlaf"/>
		<rdfs:seeAlso rdf:resource="#JavaIo"/>
		<rdfs:comment xml:lang="en">Java API part implementing the javax.swing.plaf.metal package for J2SE 1.4</rdfs:comment>
	</owl:Class>
	<owl:Class rdf:about="#JavaxSwingPlafMulti">
		<rdfs:subClassOf rdf:resource="&j2se-1_3;JavaxSwingPlafMulti"/>
		<rdfs:seeAlso rdf:resource="#JavaAwt"/>
		<rdfs:seeAlso rdf:resource="#JavaLang"/>
		<rdfs:seeAlso rdf:resource="#JavaxAccessibility"/>
		<rdfs:seeAlso rdf:resource="#JavaxSwing"/>
		<rdfs:seeAlso rdf:resource="#JavaAwtEvent"/>
		<rdfs:seeAlso rdf:resource="#JavaxSwingTree"/>
		<rdfs:seeAlso rdf:resource="#JavaxSwingFilechooser"/>
		<rdfs:seeAlso rdf:resource="#JavaxSwingText"/>
		<rdfs:seeAlso rdf:resource="#JavaUtil"/>
		<rdfs:seeAlso rdf:resource="#JavaxSwingPlaf"/>
		<rdfs:seeAlso rdf:resource="#JavaIo"/>
		<rdfs:comment xml:lang="en">Java API part implementing the javax.swing.plaf.multi package for J2SE 1.4</rdfs:comment>
	</owl:Class>
	<owl:Class rdf:about="#JavaxSwingEvent">
		<rdfs:subClassOf rdf:resource="&j2se-1_3;JavaxSwingEvent"/>
		<rdfs:seeAlso rdf:resource="#JavaxSwingUndo"/>
		<rdfs:seeAlso rdf:resource="#JavaAwt"/>
		<rdfs:seeAlso rdf:resource="#JavaxSwingText"/>
		<rdfs:seeAlso rdf:resource="#JavaUtil"/>
		<rdfs:seeAlso rdf:resource="#JavaxSwingTable"/>
		<rdfs:seeAlso rdf:resource="#JavaLang"/>
		<rdfs:seeAlso rdf:resource="#JavaIo"/>
		<rdfs:seeAlso rdf:resource="#JavaNet"/>
		<rdfs:seeAlso rdf:resource="#JavaBeans"/>
		<rdfs:seeAlso rdf:resource="#JavaxSwing"/>
		<rdfs:seeAlso rdf:resource="#JavaAwtEvent"/>
		<rdfs:seeAlso rdf:resource="#JavaxSwingTree"/>
		<rdfs:comment xml:lang="en">Java API part implementing the javax.swing.event package for J2SE 1.4</rdfs:comment>
	</owl:Class>
	<owl:Class rdf:about="#JavaxSwingBorder">
		<owl:equivalentClass rdf:resource="&j2se-1_3;JavaxSwingBorder"/>
		<rdfs:subClassOf rdf:resource="&java;JavaAPIPart"/>
		<rdfs:seeAlso rdf:resource="#JavaLang"/>
		<rdfs:seeAlso rdf:resource="#JavaAwt"/>
		<rdfs:seeAlso rdf:resource="#JavaIo"/>
		<rdfs:seeAlso rdf:resource="#JavaxSwing"/>
		<rdfs:comment xml:lang="en">Java API part implementing the javax.swing.border package for J2SE 1.4</rdfs:comment>
	</owl:Class>
	<owl:Class rdf:about="#JavaxSwingText">
		<rdfs:subClassOf rdf:resource="&j2se-1_3;JavaxSwingText"/>
		<rdfs:seeAlso rdf:resource="#JavaAwt"/>
		<rdfs:seeAlso rdf:resource="#JavaLang"/>
		<rdfs:seeAlso rdf:resource="#JavaxSwingPlafBasic"/>
		<rdfs:seeAlso rdf:resource="#JavaxSwingEvent"/>
		<rdfs:seeAlso rdf:resource="#JavaxAccessibility"/>
		<rdfs:seeAlso rdf:resource="#JavaxSwing"/>
		<rdfs:seeAlso rdf:resource="#JavaAwtEvent"/>
		<rdfs:seeAlso rdf:resource="#JavaxSwingTree"/>
		<rdfs:seeAlso rdf:resource="#JavaxSwingUndo"/>
		<rdfs:seeAlso rdf:resource="#JavaUtil"/>
		<rdfs:seeAlso rdf:resource="#JavaxSwingPlaf"/>
		<rdfs:seeAlso rdf:resource="#JavaIo"/>
		<rdfs:seeAlso rdf:resource="#JavaText"/>
		<rdfs:seeAlso rdf:resource="#JavaAwtIm"/>
		<rdfs:comment xml:lang="en">Java API part implementing the javax.swing.text package for J2SE 1.4</rdfs:comment>
	</owl:Class>
	<owl:Class rdf:about="#JavaxSwingTextHtml">
		<rdfs:subClassOf rdf:resource="&j2se-1_3;JavaxSwingTextHtml"/>
		<rdfs:seeAlso rdf:resource="#JavaAwt"/>
		<rdfs:seeAlso rdf:resource="#JavaLang"/>
		<rdfs:seeAlso rdf:resource="#JavaNet"/>
		<rdfs:seeAlso rdf:resource="#JavaxSwingEvent"/>
		<rdfs:seeAlso rdf:resource="#JavaxAccessibility"/>
		<rdfs:seeAlso rdf:resource="#JavaxSwing"/>
		<rdfs:seeAlso rdf:resource="#JavaAwtEvent"/>
		<rdfs:seeAlso rdf:resource="#JavaxSwingText"/>
		<rdfs:seeAlso rdf:resource="#JavaUtil"/>
		<rdfs:seeAlso rdf:resource="#JavaIo"/>
		<rdfs:comment xml:lang="en">Java API part implementing the javax.swing.text.html package for J2SE 1.4</rdfs:comment>
	</owl:Class>
	<owl:Class rdf:about="#JavaxSwingTextHtmlParser">
		<owl:equivalentClass rdf:resource="&j2se-1_3;JavaxSwingTextHtmlParser"/>
		<rdfs:subClassOf rdf:resource="&java;JavaAPIPart"/>
		<rdfs:seeAlso rdf:resource="#JavaxSwingTextHtml"/>
		<rdfs:seeAlso rdf:resource="#JavaxSwingText"/>
		<rdfs:seeAlso rdf:resource="#JavaUtil"/>
		<rdfs:seeAlso rdf:resource="#JavaLang"/>
		<rdfs:seeAlso rdf:resource="#JavaIo"/>
		<rdfs:comment xml:lang="en">Java API part implementing the javax.swing.text.html.parser package for J2SE 1.4</rdfs:comment>
	</owl:Class>
	<owl:Class rdf:about="#JavaxSwingTextRtf">
		<owl:equivalentClass rdf:resource="&j2se-1_3;JavaxSwingTextRtf"/>
		<rdfs:subClassOf rdf:resource="&java;JavaAPIPart"/>
		<rdfs:seeAlso rdf:resource="#JavaLang"/>
		<rdfs:seeAlso rdf:resource="#JavaIo"/>
		<rdfs:seeAlso rdf:resource="#JavaxSwingText"/>
		<rdfs:comment xml:lang="en">Java API part implementing the javax.swing.text.rtf package for J2SE 1.4</rdfs:comment>
	</owl:Class>
	<owl:Class rdf:about="#JavaxSwingTable">
		<rdfs:subClassOf rdf:resource="&j2se-1_3;JavaxSwingTable"/>
		<rdfs:seeAlso rdf:resource="#JavaAwt"/>
		<rdfs:seeAlso rdf:resource="#JavaUtil"/>
		<rdfs:seeAlso rdf:resource="#JavaLang"/>
		<rdfs:seeAlso rdf:resource="#JavaxSwingPlaf"/>
		<rdfs:seeAlso rdf:resource="#JavaIo"/>
		<rdfs:seeAlso rdf:resource="#JavaxSwingEvent"/>
		<rdfs:seeAlso rdf:resource="#JavaxSwingBorder"/>
		<rdfs:seeAlso rdf:resource="#JavaBeans"/>
		<rdfs:seeAlso rdf:resource="#JavaxAccessibility"/>
		<rdfs:seeAlso rdf:resource="#JavaxSwing"/>
		<rdfs:seeAlso rdf:resource="#JavaAwtEvent"/>
		<rdfs:comment xml:lang="en">Java API part implementing the javax.swing.table package for J2SE 1.4</rdfs:comment>
	</owl:Class>
	<owl:Class rdf:about="#JavaxSwingUndo">
		<rdfs:subClassOf rdf:resource="&j2se-1_3;JavaxSwingUndo"/>
		<rdfs:seeAlso rdf:resource="#JavaUtil"/>
		<rdfs:seeAlso rdf:resource="#JavaxSwingEvent"/>
		<rdfs:seeAlso rdf:resource="#JavaLang"/>
		<rdfs:seeAlso rdf:resource="#JavaIo"/>
		<rdfs:comment xml:lang="en">Java API part implementing the javax.swing.undo package for J2SE 1.4</rdfs:comment>
	</owl:Class>
	<owl:Class rdf:about="#JavaxSwingTree">
		<rdfs:subClassOf rdf:resource="&j2se-1_3;JavaxSwingTree"/>
		<rdfs:seeAlso rdf:resource="#JavaAwt"/>
		<rdfs:seeAlso rdf:resource="#JavaUtil"/>
		<rdfs:seeAlso rdf:resource="#JavaLang"/>
		<rdfs:seeAlso rdf:resource="#JavaIo"/>
		<rdfs:seeAlso rdf:resource="#JavaxSwingEvent"/>
		<rdfs:seeAlso rdf:resource="#JavaxSwingBorder"/>
		<rdfs:seeAlso rdf:resource="#JavaBeans"/>
		<rdfs:seeAlso rdf:resource="#JavaxSwing"/>
		<rdfs:seeAlso rdf:resource="#JavaAwtEvent"/>
		<rdfs:comment xml:lang="en">Java API part implementing the javax.swing.tree package for J2SE 1.4</rdfs:comment>
	</owl:Class>
	<owl:Class rdf:about="#JavaxSwingFilechooser">
		<rdfs:subClassOf rdf:resource="&j2se-1_3;JavaxSwingFilechooser"/>
		<rdfs:seeAlso rdf:resource="#JavaLang"/>
		<rdfs:seeAlso rdf:resource="#JavaIo"/>
		<rdfs:seeAlso rdf:resource="#JavaxSwing"/>
		<rdfs:comment xml:lang="en">Java API part implementing the javax.swing.filechooser package for J2SE 1.4</rdfs:comment>
	</owl:Class>
	<owl:Class rdf:about="#JavaxSwingColorchooser">
		<rdfs:subClassOf rdf:resource="&j2se-1_3;JavaxSwingColorchooser"/>
		<rdfs:seeAlso rdf:resource="#JavaxSwingEvent"/>
		<rdfs:seeAlso rdf:resource="#JavaAwt"/>
		<rdfs:seeAlso rdf:resource="#JavaxSwing"/>
		<rdfs:seeAlso rdf:resource="#JavaLang"/>
		<rdfs:seeAlso rdf:resource="#JavaIo"/>
		<rdfs:comment xml:lang="en">Java API part implementing the javax.swing.colorchooser package for J2SE 1.4</rdfs:comment>
	</owl:Class>
	<owl:Class rdf:about="#JavaxSoundSampled">
		<rdfs:subClassOf rdf:resource="&j2se-1_3;JavaxSoundSampled"/>
		<rdfs:seeAlso rdf:resource="#JavaNet"/>
		<rdfs:seeAlso rdf:resource="#JavaSecurity"/>
		<rdfs:seeAlso rdf:resource="#JavaUtil"/>
		<rdfs:seeAlso rdf:resource="#JavaLang"/>
		<rdfs:seeAlso rdf:resource="#JavaIo"/>
		<rdfs:comment xml:lang="en">Java API part implementing the javax.sound.sampled package for J2SE 1.4</rdfs:comment>
	</owl:Class>
	<owl:Class rdf:about="#JavaxSoundSampledSpi">
		<owl:equivalentClass rdf:resource="&j2se-1_3;JavaxSoundSampledSpi"/>
		<rdfs:subClassOf rdf:resource="&java;JavaAPIPart"/>
		<rdfs:seeAlso rdf:resource="#JavaNet"/>
		<rdfs:seeAlso rdf:resource="#JavaxSoundSampled"/>
		<rdfs:seeAlso rdf:resource="#JavaLang"/>
		<rdfs:seeAlso rdf:resource="#JavaIo"/>
		<rdfs:comment xml:lang="en">Java API part implementing the javax.sound.sampled.spi package for J2SE 1.4</rdfs:comment>
	</owl:Class>
	<owl:Class rdf:about="#JavaxSoundMidi">
		<rdfs:subClassOf rdf:resource="&j2se-1_3;JavaxSoundMidi"/>
		<rdfs:seeAlso rdf:resource="#JavaNet"/>
		<rdfs:seeAlso rdf:resource="#JavaUtil"/>
		<rdfs:seeAlso rdf:resource="#JavaLang"/>
		<rdfs:seeAlso rdf:resource="#JavaIo"/>
		<rdfs:comment xml:lang="en">Java API part implementing the javax.sound.midi package for J2SE 1.4</rdfs:comment>
	</owl:Class>
	<owl:Class rdf:about="#JavaxSoundMidiSpi">
		<owl:equivalentClass rdf:resource="&j2se-1_3;JavaxSoundMidiSpi"/>
		<rdfs:subClassOf rdf:resource="&java;JavaAPIPart"/>
		<rdfs:seeAlso rdf:resource="#JavaNet"/>
		<rdfs:seeAlso rdf:resource="#JavaLang"/>
		<rdfs:seeAlso rdf:resource="#JavaIo"/>
		<rdfs:seeAlso rdf:resource="#JavaxSoundMidi"/>
		<rdfs:comment xml:lang="en">Java API part implementing the javax.sound.midi.spi package for J2SE 1.4</rdfs:comment>
	</owl:Class>
	<owl:Class rdf:about="#JavaxPrint">
		<rdfs:subClassOf rdf:resource="&java;JavaAPIPart"/>
		<rdfs:seeAlso rdf:resource="#JavaNet"/>
		<rdfs:seeAlso rdf:resource="#JavaxPrintEvent"/>
		<rdfs:seeAlso rdf:resource="#JavaAwt"/>
		<rdfs:seeAlso rdf:resource="#JavaxPrintAttribute"/>
		<rdfs:seeAlso rdf:resource="#JavaLang"/>
		<rdfs:seeAlso rdf:resource="#JavaIo"/>
		<rdfs:comment xml:lang="en">Java API part implementing the javax.print package for J2SE 1.4</rdfs:comment>
	</owl:Class>
	<owl:Class rdf:about="#JavaxPrintAttribute">
		<rdfs:subClassOf rdf:resource="&java;JavaAPIPart"/>
		<rdfs:seeAlso rdf:resource="#JavaNet"/>
		<rdfs:seeAlso rdf:resource="#JavaUtil"/>
		<rdfs:seeAlso rdf:resource="#JavaLang"/>
		<rdfs:seeAlso rdf:resource="#JavaIo"/>
		<rdfs:comment xml:lang="en">Java API part implementing the javax.print.attribute package for J2SE 1.4</rdfs:comment>
	</owl:Class>
	<owl:Class rdf:about="#JavaxPrintAttributeStandard">
		<rdfs:subClassOf rdf:resource="&java;JavaAPIPart"/>
		<rdfs:seeAlso rdf:resource="#JavaUtil"/>
		<rdfs:seeAlso rdf:resource="#JavaLang"/>
		<rdfs:seeAlso rdf:resource="#JavaNet"/>
		<rdfs:seeAlso rdf:resource="#JavaxPrintAttribute"/>
		<rdfs:comment xml:lang="en">Java API part implementing the javax.print.attribute.standard package for J2SE 1.4</rdfs:comment>
	</owl:Class>
	<owl:Class rdf:about="#JavaxPrintEvent">
		<rdfs:subClassOf rdf:resource="&java;JavaAPIPart"/>
		<rdfs:seeAlso rdf:resource="#JavaUtil"/>
		<rdfs:seeAlso rdf:resource="#JavaLang"/>
		<rdfs:seeAlso rdf:resource="#JavaxPrintAttribute"/>
		<rdfs:seeAlso rdf:resource="#JavaxPrint"/>
		<rdfs:comment xml:lang="en">Java API part implementing the javax.print.event package for J2SE 1.4</rdfs:comment>
	</owl:Class>
	<owl:Class rdf:about="#JavaxSecurityAuth">
		<rdfs:subClassOf rdf:resource="&java;JavaAPIPart"/>
		<rdfs:seeAlso rdf:resource="#JavaUtil"/>
		<rdfs:seeAlso rdf:resource="#JavaSecurity"/>
		<rdfs:seeAlso rdf:resource="#JavaLang"/>
		<rdfs:seeAlso rdf:resource="#JavaIo"/>
		<rdfs:comment xml:lang="en">Java API part implementing the javax.security.auth package for J2SE 1.4</rdfs:comment>
	</owl:Class>
	<owl:Class rdf:about="#JavaxSecurityAuthX500">
		<rdfs:subClassOf rdf:resource="&j2me-pp-1_1;JavaxSecurityAuthX500"/>
		<rdfs:seeAlso rdf:resource="#JavaSecurity"/>
		<rdfs:seeAlso rdf:resource="#JavaLang"/>
		<rdfs:seeAlso rdf:resource="#JavaSecurityCert"/>
		<rdfs:seeAlso rdf:resource="#JavaIo"/>
		<rdfs:seeAlso rdf:resource="#JavaxSecurityAuth"/>
		<rdfs:comment xml:lang="en">Java API part implementing the javax.security.auth.x500 package for J2SE 1.4</rdfs:comment>
	</owl:Class>
	<owl:Class rdf:about="#JavaxSecurityAuthCallback">
		<rdfs:subClassOf rdf:resource="&java;JavaAPIPart"/>
		<rdfs:seeAlso rdf:resource="#JavaUtil"/>
		<rdfs:seeAlso rdf:resource="#JavaLang"/>
		<rdfs:seeAlso rdf:resource="#JavaIo"/>
		<rdfs:comment xml:lang="en">Java API part implementing the javax.security.auth.callback package for J2SE 1.4</rdfs:comment>
	</owl:Class>
	<owl:Class rdf:about="#JavaxSecurityAuthKerberos">
		<rdfs:subClassOf rdf:resource="&java;JavaAPIPart"/>
		<rdfs:seeAlso rdf:resource="#JavaUtil"/>
		<rdfs:seeAlso rdf:resource="#JavaSecurity"/>
		<rdfs:seeAlso rdf:resource="#JavaLang"/>
		<rdfs:seeAlso rdf:resource="#JavaxCrypto"/>
		<rdfs:seeAlso rdf:resource="#JavaIo"/>
		<rdfs:seeAlso rdf:resource="#JavaxSecurityAuth"/>
		<rdfs:comment xml:lang="en">Java API part implementing the javax.security.auth.kerberos package for J2SE 1.4</rdfs:comment>
	</owl:Class>
	<owl:Class rdf:about="#JavaxSecurityAuthLogin">
		<rdfs:subClassOf rdf:resource="&java;JavaAPIPart"/>
		<rdfs:seeAlso rdf:resource="#JavaSecurity"/>
		<rdfs:seeAlso rdf:resource="#JavaUtil"/>
		<rdfs:seeAlso rdf:resource="#JavaxSecurityAuthCallback"/>
		<rdfs:seeAlso rdf:resource="#JavaLang"/>
		<rdfs:seeAlso rdf:resource="#JavaxSecurityAuth"/>
		<rdfs:comment xml:lang="en">Java API part implementing the javax.security.auth.login package for J2SE 1.4</rdfs:comment>
	</owl:Class>
	<owl:Class rdf:about="#JavaxSecurityAuthSpi">
		<rdfs:subClassOf rdf:resource="&java;JavaAPIPart"/>
		<rdfs:seeAlso rdf:resource="#JavaUtil"/>
		<rdfs:seeAlso rdf:resource="#JavaxSecurityAuthCallback"/>
		<rdfs:seeAlso rdf:resource="#JavaxSecurityAuth"/>
		<rdfs:comment xml:lang="en">Java API part implementing the javax.security.auth.spi package for J2SE 1.4</rdfs:comment>
	</owl:Class>
	<owl:Class rdf:about="#JavaxSecurityCert">
		<rdfs:subClassOf rdf:resource="&java;JavaAPIPart"/>
		<rdfs:seeAlso rdf:resource="#JavaSecurity"/>
		<rdfs:seeAlso rdf:resource="#JavaUtil"/>
		<rdfs:seeAlso rdf:resource="#JavaLang"/>
		<rdfs:seeAlso rdf:resource="#JavaIo"/>
		<rdfs:seeAlso rdf:resource="#JavaMath"/>
		<rdfs:comment xml:lang="en">Java API part implementing the javax.security.cert package for J2SE 1.4</rdfs:comment>
	</owl:Class>
	<owl:Class rdf:about="#JavaxNaming">
		<rdfs:subClassOf rdf:resource="&j2se-1_3;JavaxNaming"/>
		<rdfs:seeAlso rdf:resource="#JavaUtil"/>
		<rdfs:seeAlso rdf:resource="#JavaLang"/>
		<rdfs:seeAlso rdf:resource="#JavaIo"/>
		<rdfs:comment xml:lang="en">Java API part implementing the javax.naming package for J2SE 1.4</rdfs:comment>
	</owl:Class>
	<owl:Class rdf:about="#JavaxNamingDirectory">
		<rdfs:subClassOf rdf:resource="&j2se-1_3;JavaxNamingDirectory"/>
		<rdfs:seeAlso rdf:resource="#JavaUtil"/>
		<rdfs:seeAlso rdf:resource="#JavaxNaming"/>
		<rdfs:seeAlso rdf:resource="#JavaLang"/>
		<rdfs:seeAlso rdf:resource="#JavaIo"/>
		<rdfs:comment xml:lang="en">Java API part implementing the javax.naming.directory package for J2SE 1.4</rdfs:comment>
	</owl:Class>
	<owl:Class rdf:about="#JavaxNamingEvent">
		<owl:equivalentClass rdf:resource="&j2se-1_3;JavaxNamingEvent"/>
		<rdfs:subClassOf rdf:resource="&java;JavaAPIPart"/>
		<rdfs:seeAlso rdf:resource="#JavaUtil"/>
		<rdfs:seeAlso rdf:resource="#JavaxNaming"/>
		<rdfs:seeAlso rdf:resource="#JavaLang"/>
		<rdfs:seeAlso rdf:resource="#JavaxNamingDirectory"/>
		<rdfs:comment xml:lang="en">Java API part implementing the javax.naming.event package for J2SE 1.4</rdfs:comment>
	</owl:Class>
	<owl:Class rdf:about="#JavaxNamingLdap">
		<rdfs:subClassOf rdf:resource="&j2se-1_3;JavaxNamingLdap"/>
		<rdfs:seeAlso rdf:resource="#JavaxNamingEvent"/>
		<rdfs:seeAlso rdf:resource="#JavaxNetSsl"/>
		<rdfs:seeAlso rdf:resource="#JavaUtil"/>
		<rdfs:seeAlso rdf:resource="#JavaxNaming"/>
		<rdfs:seeAlso rdf:resource="#JavaLang"/>
		<rdfs:seeAlso rdf:resource="#JavaxNamingDirectory"/>
		<rdfs:seeAlso rdf:resource="#JavaIo"/>
		<rdfs:comment xml:lang="en">Java API part implementing the javax.naming.ldap package for J2SE 1.4</rdfs:comment>
	</owl:Class>
	<owl:Class rdf:about="#JavaxNamingSpi">
		<owl:equivalentClass rdf:resource="&j2se-1_3;JavaxNamingSpi"/>
		<rdfs:subClassOf rdf:resource="&java;JavaAPIPart"/>
		<rdfs:seeAlso rdf:resource="#JavaUtil"/>
		<rdfs:seeAlso rdf:resource="#JavaxNaming"/>
		<rdfs:seeAlso rdf:resource="#JavaLang"/>
		<rdfs:seeAlso rdf:resource="#JavaxNamingDirectory"/>
		<rdfs:seeAlso rdf:resource="#JavaIo"/>
		<rdfs:comment xml:lang="en">Java API part implementing the javax.naming.spi package for J2SE 1.4</rdfs:comment>
	</owl:Class>
	<owl:Class rdf:about="#JavaxNet">
		<rdfs:subClassOf rdf:resource="&java;JavaAPIPart"/>
		<rdfs:seeAlso rdf:resource="#JavaNet"/>
		<rdfs:seeAlso rdf:resource="#JavaLang"/>
		<rdfs:comment xml:lang="en">Java API part implementing the javax.net package for J2SE 1.4</rdfs:comment>
	</owl:Class>
	<owl:Class rdf:about="#JavaxNetSsl">
		<rdfs:subClassOf rdf:resource="&java;JavaAPIPart"/>
		<rdfs:seeAlso rdf:resource="#JavaNet"/>
		<rdfs:seeAlso rdf:resource="#JavaUtil"/>
		<rdfs:seeAlso rdf:resource="#JavaSecurity"/>
		<rdfs:seeAlso rdf:resource="#JavaLang"/>
		<rdfs:seeAlso rdf:resource="#JavaIo"/>
		<rdfs:seeAlso rdf:resource="#JavaxNet"/>
		<rdfs:comment xml:lang="en">Java API part implementing the javax.net.ssl package for J2SE 1.4</rdfs:comment>
	</owl:Class>
	<owl:Class rdf:about="#JavaxRmi">
		<owl:equivalentClass rdf:resource="&j2se-1_3;JavaxRmi"/>
		<rdfs:subClassOf rdf:resource="&java;JavaAPIPart"/>
		<rdfs:seeAlso rdf:resource="#JavaLang"/>
		<rdfs:seeAlso rdf:resource="#JavaRmi"/>
		<rdfs:comment xml:lang="en">Java API part implementing the javax.rmi package for J2SE 1.4</rdfs:comment>
	</owl:Class>
	<owl:Class rdf:about="#JavaxRmiCORBA">
		<owl:equivalentClass rdf:resource="&j2se-1_3;JavaxRmiCORBA"/>
		<rdfs:subClassOf rdf:resource="&java;JavaAPIPart"/>
		<rdfs:seeAlso rdf:resource="#OrgOmgCORBA_2_3Portable"/>
		<rdfs:seeAlso rdf:resource="#OrgOmgCORBA"/>
		<rdfs:seeAlso rdf:resource="#OrgOmgSendingContext"/>
		<rdfs:seeAlso rdf:resource="#OrgOmgCORBAPortable"/>
		<rdfs:seeAlso rdf:resource="#JavaLang"/>
		<rdfs:seeAlso rdf:resource="#JavaIo"/>
		<rdfs:seeAlso rdf:resource="#JavaRmi"/>
		<rdfs:comment xml:lang="en">Java API part implementing the javax.rmi.CORBA package for J2SE 1.4</rdfs:comment>
	</owl:Class>
	<owl:Class rdf:about="#JavaxCrypto">
		<rdfs:subClassOf rdf:resource="&java;JavaAPIPart"/>
		<rdfs:seeAlso rdf:resource="#JavaSecurityCert"/>
		<rdfs:seeAlso rdf:resource="#JavaSecurity"/>
		<rdfs:seeAlso rdf:resource="#JavaSecuritySpec"/>
		<rdfs:seeAlso rdf:resource="#JavaLang"/>
		<rdfs:seeAlso rdf:resource="#JavaIo"/>
		<rdfs:comment xml:lang="en">Java API part implementing the javax.crypto package for J2SE 1.4</rdfs:comment>
	</owl:Class>
	<owl:Class rdf:about="#JavaxCryptoInterfaces">
		<rdfs:subClassOf rdf:resource="&java;JavaAPIPart"/>
		<rdfs:seeAlso rdf:resource="#JavaSecurity"/>
		<rdfs:seeAlso rdf:resource="#JavaxCrypto"/>
		<rdfs:seeAlso rdf:resource="#JavaxCryptoSpec"/>
		<rdfs:seeAlso rdf:resource="#JavaMath"/>
		<rdfs:comment xml:lang="en">Java API part implementing the javax.crypto.interfaces package for J2SE 1.4</rdfs:comment>
	</owl:Class>
	<owl:Class rdf:about="#JavaxCryptoSpec">
		<rdfs:subClassOf rdf:resource="&java;JavaAPIPart"/>
		<rdfs:seeAlso rdf:resource="#JavaSecuritySpec"/>
		<rdfs:seeAlso rdf:resource="#JavaLang"/>
		<rdfs:seeAlso rdf:resource="#JavaxCrypto"/>
		<rdfs:seeAlso rdf:resource="#JavaMath"/>
		<rdfs:comment xml:lang="en">Java API part implementing the javax.crypto.spec package for J2SE 1.4</rdfs:comment>
	</owl:Class>
	<owl:Class rdf:about="#JavaxSql">
		<rdfs:subClassOf rdf:resource="&java;JavaAPIPart"/>
		<rdfs:seeAlso rdf:resource="#JavaxTransactionXa"/>
		<rdfs:seeAlso rdf:resource="#JavaSql"/>
		<rdfs:seeAlso rdf:resource="#JavaMath"/>
		<rdfs:seeAlso rdf:resource="#JavaUtil"/>
		<rdfs:seeAlso rdf:resource="#JavaLang"/>
		<rdfs:seeAlso rdf:resource="#JavaIo"/>
		<rdfs:comment xml:lang="en">Java API part implementing the javax.sql package for J2SE 1.4</rdfs:comment>
	</owl:Class>
	<owl:Class rdf:about="#JavaxTransaction">
		<rdfs:subClassOf rdf:resource="&j2se-1_3;JavaxTransaction"/>
		<rdfs:seeAlso rdf:resource="#JavaLang"/>
		<rdfs:seeAlso rdf:resource="#JavaRmi"/>
		<rdfs:comment xml:lang="en">Java API part implementing the javax.transaction package for J2SE 1.4</rdfs:comment>
	</owl:Class>
	<owl:Class rdf:about="#JavaxTransactionXa">
		<rdfs:subClassOf rdf:resource="&java;JavaAPIPart"/>
		<rdfs:seeAlso rdf:resource="#JavaLang"/>
		<rdfs:comment xml:lang="en">Java API part implementing the javax.transaction.xa package for J2SE 1.4</rdfs:comment>
	</owl:Class>
	<owl:Class rdf:about="#JavaxXmlParsers">
		<rdfs:subClassOf rdf:resource="&java;JavaAPIPart"/>
		<rdfs:seeAlso rdf:resource="#OrgXmlSax"/>
		<rdfs:seeAlso rdf:resource="#OrgXmlSaxHelpers"/>
		<rdfs:seeAlso rdf:resource="#OrgW3cDom"/>
		<rdfs:seeAlso rdf:resource="#JavaLang"/>
		<rdfs:seeAlso rdf:resource="#JavaIo"/>
		<rdfs:comment xml:lang="en">Java API part implementing the javax.xml.parsers package for J2SE 1.4</rdfs:comment>
	</owl:Class>
	<owl:Class rdf:about="#JavaxXmlTransform">
		<rdfs:subClassOf rdf:resource="&java;JavaAPIPart"/>
		<rdfs:seeAlso rdf:resource="#JavaUtil"/>
		<rdfs:seeAlso rdf:resource="#JavaLang"/>
		<rdfs:seeAlso rdf:resource="#JavaIo"/>
		<rdfs:comment xml:lang="en">Java API part implementing the javax.xml.transform package for J2SE 1.4</rdfs:comment>
	</owl:Class>
	<owl:Class rdf:about="#JavaxXmlTransformDom">
		<rdfs:subClassOf rdf:resource="&java;JavaAPIPart"/>
		<rdfs:seeAlso rdf:resource="#JavaLang"/>
		<rdfs:seeAlso rdf:resource="#JavaxXmlTransform"/>
		<rdfs:seeAlso rdf:resource="#OrgW3cDom"/>
		<rdfs:comment xml:lang="en">Java API part implementing the javax.xml.transform.dom package for J2SE 1.4</rdfs:comment>
	</owl:Class>
	<owl:Class rdf:about="#JavaxXmlTransformSax">
		<rdfs:subClassOf rdf:resource="&java;JavaAPIPart"/>
		<rdfs:seeAlso rdf:resource="#OrgXmlSax"/>
		<rdfs:seeAlso rdf:resource="#JavaxXmlTransform"/>
		<rdfs:seeAlso rdf:resource="#JavaLang"/>
		<rdfs:seeAlso rdf:resource="#OrgXmlSaxExt"/>
		<rdfs:comment xml:lang="en">Java API part implementing the javax.xml.transform.sax package for J2SE 1.4</rdfs:comment>
	</owl:Class>
	<owl:Class rdf:about="#JavaxXmlTransformStream">
		<rdfs:subClassOf rdf:resource="&java;JavaAPIPart"/>
		<rdfs:seeAlso rdf:resource="#JavaLang"/>
		<rdfs:seeAlso rdf:resource="#JavaIo"/>
		<rdfs:seeAlso rdf:resource="#JavaxXmlTransform"/>
		<rdfs:comment xml:lang="en">Java API part implementing the javax.xml.transform.stream package for J2SE 1.4</rdfs:comment>
	</owl:Class>
	<owl:Class rdf:about="#OrgW3cDom">
		<rdfs:subClassOf rdf:resource="&java;JavaAPIPart"/>
		<rdfs:seeAlso rdf:resource="#JavaLang"/>
		<rdfs:comment xml:lang="en">Java API part implementing the org.w3c.dom package for J2SE 1.4</rdfs:comment>
	</owl:Class>
	<owl:Class rdf:about="#OrgW3cDomCss">
		<rdfs:subClassOf rdf:resource="&java;JavaAPIPart"/>
		<rdfs:seeAlso rdf:resource="#JavaLang"/>
		<rdfs:seeAlso rdf:resource="#OrgW3cDomViews"/>
		<rdfs:seeAlso rdf:resource="#OrgW3cDom"/>
		<rdfs:seeAlso rdf:resource="#OrgW3cDomStylesheets"/>
		<rdfs:comment xml:lang="en">Java API part implementing the org.w3c.dom.css package for J2SE 1.4</rdfs:comment>
	</owl:Class>
	<owl:Class rdf:about="#OrgW3cDomStylesheets">
		<rdfs:subClassOf rdf:resource="&java;JavaAPIPart"/>
		<rdfs:seeAlso rdf:resource="#JavaLang"/>
		<rdfs:seeAlso rdf:resource="#OrgW3cDom"/>
		<rdfs:comment xml:lang="en">Java API part implementing the org.w3c.dom.stylesheets package for J2SE 1.4</rdfs:comment>
	</owl:Class>
	<owl:Class rdf:about="#OrgW3cDomViews">
		<rdfs:subClassOf rdf:resource="&java;JavaAPIPart"/>
		<rdfs:comment xml:lang="en">Java API part implementing the org.w3c.dom.views package for J2SE 1.4</rdfs:comment>
	</owl:Class>
	<owl:Class rdf:about="#OrgW3cDomEvents">
		<rdfs:subClassOf rdf:resource="&java;JavaAPIPart"/>
		<rdfs:seeAlso rdf:resource="#JavaLang"/>
		<rdfs:seeAlso rdf:resource="#OrgW3cDomViews"/>
		<rdfs:seeAlso rdf:resource="#OrgW3cDom"/>
		<rdfs:comment xml:lang="en">Java API part implementing the org.w3c.dom.events package for J2SE 1.4</rdfs:comment>
	</owl:Class>
	<owl:Class rdf:about="#OrgW3cDomHtml">
		<rdfs:subClassOf rdf:resource="&java;JavaAPIPart"/>
		<rdfs:seeAlso rdf:resource="#JavaLang"/>
		<rdfs:seeAlso rdf:resource="#OrgW3cDom"/>
		<rdfs:comment xml:lang="en">Java API part implementing the org.w3c.dom.html package for J2SE 1.4</rdfs:comment>
	</owl:Class>
	<owl:Class rdf:about="#OrgW3cDomTraversal">
		<rdfs:subClassOf rdf:resource="&java;JavaAPIPart"/>
		<rdfs:seeAlso rdf:resource="#OrgW3cDom"/>
		<rdfs:comment xml:lang="en">Java API part implementing the org.w3c.dom.traversal package for J2SE 1.4</rdfs:comment>
	</owl:Class>
	<owl:Class rdf:about="#OrgOmgCORBA_2_3">
		<owl:equivalentClass rdf:resource="&j2se-1_3;OrgOmgCORBA_2_3"/>
		<rdfs:subClassOf rdf:resource="&java;JavaAPIPart"/>
		<rdfs:seeAlso rdf:resource="#OrgOmgCORBAPortable"/>
		<rdfs:seeAlso rdf:resource="#JavaLang"/>
		<rdfs:seeAlso rdf:resource="#OrgOmgCORBA"/>
		<rdfs:comment xml:lang="en">Java API part implementing the org.omg.CORBA_2_3 package for J2SE 1.4</rdfs:comment>
	</owl:Class>
	<owl:Class rdf:about="#OrgOmgCORBA_2_3Portable">
		<rdfs:subClassOf rdf:resource="&java;JavaAPIPart"/>
		<rdfs:seeAlso rdf:resource="#JavaLang"/>
		<rdfs:seeAlso rdf:resource="#OrgOmgCORBAPortable"/>
		<rdfs:seeAlso rdf:resource="#OrgOmgCORBA"/>
		<rdfs:seeAlso rdf:resource="#JavaIo"/>
		<rdfs:comment xml:lang="en">Java API part implementing the org.omg.CORBA_2_3.portable package for J2SE 1.4</rdfs:comment>
	</owl:Class>
	<owl:Class rdf:about="#OrgOmgCORBA">
		<rdfs:subClassOf rdf:resource="&java;JavaAPIPart"/>
		<rdfs:seeAlso rdf:resource="#JavaMath"/>
		<rdfs:seeAlso rdf:resource="#JavaApplet"/>
		<rdfs:seeAlso rdf:resource="#JavaUtil"/>
		<rdfs:seeAlso rdf:resource="#JavaLang"/>
		<rdfs:seeAlso rdf:resource="#OrgOmgCORBAPortable"/>
		<rdfs:seeAlso rdf:resource="#JavaIo"/>
		<rdfs:comment xml:lang="en">Java API part implementing the org.omg.CORBA package for J2SE 1.4</rdfs:comment>
	</owl:Class>
	<owl:Class rdf:about="#OrgOmgCORBAPortable">
		<rdfs:subClassOf rdf:resource="&java;JavaAPIPart"/>
		<rdfs:seeAlso rdf:resource="#OrgOmgCORBA"/>
		<rdfs:seeAlso rdf:resource="#JavaMath"/>
		<rdfs:seeAlso rdf:resource="#JavaLang"/>
		<rdfs:seeAlso rdf:resource="#JavaIo"/>
		<rdfs:seeAlso rdf:resource="#OrgOmgCORBA_2_3Portable"/>
		<rdfs:comment xml:lang="en">Java API part implementing the org.omg.CORBA.portable package for J2SE 1.4</rdfs:comment>
	</owl:Class>
	<owl:Class rdf:about="#OrgOmgCORBADynAnyPackage">
		<rdfs:subClassOf rdf:resource="&j2se-1_3;OrgOmgCORBADynAnyPackage"/>
		<rdfs:seeAlso rdf:resource="#JavaLang"/>
		<rdfs:seeAlso rdf:resource="#OrgOmgCORBA"/>
		<rdfs:comment xml:lang="en">Java API part implementing the org.omg.CORBA.DynAnyPackage package for J2SE 1.4</rdfs:comment>
	</owl:Class>
	<owl:Class rdf:about="#OrgOmgCORBAORBPackage">
		<rdfs:subClassOf rdf:resource="&j2se-1_3;OrgOmgCORBAORBPackage"/>
		<rdfs:seeAlso rdf:resource="#JavaLang"/>
		<rdfs:seeAlso rdf:resource="#OrgOmgCORBA"/>
		<rdfs:comment xml:lang="en">Java API part implementing the org.omg.CORBA.ORBPackage package for J2SE 1.4</rdfs:comment>
	</owl:Class>
	<owl:Class rdf:about="#OrgOmgCORBATypeCodePackage">
		<rdfs:subClassOf rdf:resource="&j2se-1_3;OrgOmgCORBATypeCodePackage"/>
		<rdfs:seeAlso rdf:resource="#JavaLang"/>
		<rdfs:seeAlso rdf:resource="#OrgOmgCORBA"/>
		<rdfs:comment xml:lang="en">Java API part implementing the org.omg.CORBA.TypeCodePackage package for J2SE 1.4</rdfs:comment>
	</owl:Class>
	<owl:Class rdf:about="#OrgOmgSendingContext">
		<owl:equivalentClass rdf:resource="&j2se-1_3;OrgOmgSendingContext"/>
		<rdfs:subClassOf rdf:resource="&java;JavaAPIPart"/>
		<rdfs:seeAlso rdf:resource="#OrgOmgCORBAPortable"/>
		<rdfs:seeAlso rdf:resource="#OrgOmgCORBA"/>
		<rdfs:comment xml:lang="en">Java API part implementing the org.omg.SendingContext package for J2SE 1.4</rdfs:comment>
	</owl:Class>
	<owl:Class rdf:about="#OrgOmgCosNaming">
		<rdfs:subClassOf rdf:resource="&java;JavaAPIPart"/>
		<rdfs:seeAlso rdf:resource="#OrgOmgCORBA"/>
		<rdfs:seeAlso rdf:resource="#OrgOmgPortableServer"/>
		<rdfs:seeAlso rdf:resource="#JavaLang"/>
		<rdfs:seeAlso rdf:resource="#OrgOmgCORBAPortable"/>
		<rdfs:comment xml:lang="en">Java API part implementing the org.omg.CosNaming package for J2SE 1.4</rdfs:comment>
	</owl:Class>
	<owl:Class rdf:about="#OrgOmgCosNamingNamingContextExtPackage">
		<rdfs:subClassOf rdf:resource="&java;JavaAPIPart"/>
		<rdfs:seeAlso rdf:resource="#OrgOmgCORBAPortable"/>
		<rdfs:seeAlso rdf:resource="#JavaLang"/>
		<rdfs:seeAlso rdf:resource="#OrgOmgCORBA"/>
		<rdfs:comment xml:lang="en">Java API part implementing the org.omg.CosNaming.NamingContextExtPackage package for J2SE 1.4</rdfs:comment>
	</owl:Class>
	<owl:Class rdf:about="#OrgOmgCosNamingNamingContextPackage">
		<rdfs:subClassOf rdf:resource="&java;JavaAPIPart"/>
		<rdfs:seeAlso rdf:resource="#OrgOmgCORBAPortable"/>
		<rdfs:seeAlso rdf:resource="#JavaLang"/>
		<rdfs:seeAlso rdf:resource="#OrgOmgCORBA"/>
		<rdfs:seeAlso rdf:resource="#OrgOmgCosNaming"/>
		<rdfs:comment xml:lang="en">Java API part implementing the org.omg.CosNaming.NamingContextPackage package for J2SE 1.4</rdfs:comment>
	</owl:Class>
	<owl:Class rdf:about="#OrgOmgPortableServer">
		<rdfs:subClassOf rdf:resource="&java;JavaAPIPart"/>
		<rdfs:seeAlso rdf:resource="#OrgOmgPortableServerPOAManagerPackage"/>
		<rdfs:seeAlso rdf:resource="#OrgOmgPortableServerPortable"/>
		<rdfs:seeAlso rdf:resource="#OrgOmgCORBA"/>
		<rdfs:seeAlso rdf:resource="#JavaLang"/>
		<rdfs:seeAlso rdf:resource="#OrgOmgCORBAPortable"/>
		<rdfs:seeAlso rdf:resource="#OrgOmgPortableServerServantLocatorPackage"/>
		<rdfs:comment xml:lang="en">Java API part implementing the org.omg.PortableServer package for J2SE 1.4</rdfs:comment>
	</owl:Class>
	<owl:Class rdf:about="#OrgOmgPortableServerCurrentPackage">
		<rdfs:subClassOf rdf:resource="&java;JavaAPIPart"/>
		<rdfs:seeAlso rdf:resource="#OrgOmgCORBAPortable"/>
		<rdfs:seeAlso rdf:resource="#JavaLang"/>
		<rdfs:seeAlso rdf:resource="#OrgOmgCORBA"/>
		<rdfs:comment xml:lang="en">Java API part implementing the org.omg.PortableServer.CurrentPackage package for J2SE 1.4</rdfs:comment>
	</owl:Class>
	<owl:Class rdf:about="#OrgOmgPortableServerPOAManagerPackage">
		<rdfs:subClassOf rdf:resource="&java;JavaAPIPart"/>
		<rdfs:seeAlso rdf:resource="#JavaLang"/>
		<rdfs:seeAlso rdf:resource="#OrgOmgCORBAPortable"/>
		<rdfs:seeAlso rdf:resource="#OrgOmgCORBA"/>
		<rdfs:comment xml:lang="en">Java API part implementing the org.omg.PortableServer.POAManagerPackage package for J2SE 1.4</rdfs:comment>
	</owl:Class>
	<owl:Class rdf:about="#OrgOmgPortableServerPOAPackage">
		<rdfs:subClassOf rdf:resource="&java;JavaAPIPart"/>
		<rdfs:seeAlso rdf:resource="#OrgOmgCORBAPortable"/>
		<rdfs:seeAlso rdf:resource="#JavaLang"/>
		<rdfs:seeAlso rdf:resource="#OrgOmgCORBA"/>
		<rdfs:comment xml:lang="en">Java API part implementing the org.omg.PortableServer.POAPackage package for J2SE 1.4</rdfs:comment>
	</owl:Class>
	<owl:Class rdf:about="#OrgOmgPortableServerPortable">
		<rdfs:subClassOf rdf:resource="&java;JavaAPIPart"/>
		<rdfs:seeAlso rdf:resource="#JavaLang"/>
		<rdfs:seeAlso rdf:resource="#OrgOmgCORBA"/>
		<rdfs:seeAlso rdf:resource="#OrgOmgPortableServer"/>
		<rdfs:comment xml:lang="en">Java API part implementing the org.omg.PortableServer.portable package for J2SE 1.4</rdfs:comment>
	</owl:Class>
	<owl:Class rdf:about="#OrgOmgPortableServerServantLocatorPackage">
		<rdfs:subClassOf rdf:resource="&java;JavaAPIPart"/>
		<rdfs:seeAlso rdf:resource="#OrgOmgCORBAPortable"/>
		<rdfs:seeAlso rdf:resource="#JavaLang"/>
		<rdfs:seeAlso rdf:resource="#OrgOmgCORBA"/>
		<rdfs:comment xml:lang="en">Java API part implementing the org.omg.PortableServer.ServantLocatorPackage package for J2SE 1.4</rdfs:comment>
	</owl:Class>
	<owl:Class rdf:about="#OrgOmgDynamic">
		<rdfs:subClassOf rdf:resource="&java;JavaAPIPart"/>
		<rdfs:seeAlso rdf:resource="#JavaLang"/>
		<rdfs:seeAlso rdf:resource="#OrgOmgCORBAPortable"/>
		<rdfs:seeAlso rdf:resource="#OrgOmgCORBA"/>
		<rdfs:comment xml:lang="en">Java API part implementing the org.omg.Dynamic package for J2SE 1.4</rdfs:comment>
	</owl:Class>
	<owl:Class rdf:about="#OrgOmgDynamicAny">
		<rdfs:subClassOf rdf:resource="&java;JavaAPIPart"/>
		<rdfs:seeAlso rdf:resource="#OrgOmgCORBA"/>
		<rdfs:seeAlso rdf:resource="#OrgOmgCORBAPortable"/>
		<rdfs:seeAlso rdf:resource="#JavaLang"/>
		<rdfs:seeAlso rdf:resource="#JavaIo"/>
		<rdfs:comment xml:lang="en">Java API part implementing the org.omg.DynamicAny package for J2SE 1.4</rdfs:comment>
	</owl:Class>
	<owl:Class rdf:about="#OrgOmgDynamicAnyDynAnyFactoryPackage">
		<rdfs:subClassOf rdf:resource="&java;JavaAPIPart"/>
		<rdfs:seeAlso rdf:resource="#OrgOmgCORBAPortable"/>
		<rdfs:seeAlso rdf:resource="#JavaLang"/>
		<rdfs:seeAlso rdf:resource="#OrgOmgCORBA"/>
		<rdfs:comment xml:lang="en">Java API part implementing the org.omg.DynamicAny.DynAnyFactoryPackage package for J2SE 1.4</rdfs:comment>
	</owl:Class>
	<owl:Class rdf:about="#OrgOmgDynamicAnyDynAnyPackage">
		<rdfs:subClassOf rdf:resource="&java;JavaAPIPart"/>
		<rdfs:seeAlso rdf:resource="#JavaLang"/>
		<rdfs:seeAlso rdf:resource="#OrgOmgCORBAPortable"/>
		<rdfs:seeAlso rdf:resource="#OrgOmgCORBA"/>
		<rdfs:comment xml:lang="en">Java API part implementing the org.omg.DynamicAny.DynAnyPackage package for J2SE 1.4</rdfs:comment>
	</owl:Class>
	<owl:Class rdf:about="#OrgOmgIOP">
		<rdfs:subClassOf rdf:resource="&java;JavaAPIPart"/>
		<rdfs:seeAlso rdf:resource="#OrgOmgCORBAPortable"/>
		<rdfs:seeAlso rdf:resource="#JavaLang"/>
		<rdfs:seeAlso rdf:resource="#OrgOmgCORBA"/>
		<rdfs:comment xml:lang="en">Java API part implementing the org.omg.IOP package for J2SE 1.4</rdfs:comment>
	</owl:Class>
	<owl:Class rdf:about="#OrgOmgIOPCodecFactoryPackage">
		<rdfs:subClassOf rdf:resource="&java;JavaAPIPart"/>
		<rdfs:seeAlso rdf:resource="#OrgOmgCORBAPortable"/>
		<rdfs:seeAlso rdf:resource="#JavaLang"/>
		<rdfs:seeAlso rdf:resource="#OrgOmgCORBA"/>
		<rdfs:comment xml:lang="en">Java API part implementing the org.omg.IOP.CodecFactoryPackage package for J2SE 1.4</rdfs:comment>
	</owl:Class>
	<owl:Class rdf:about="#OrgOmgIOPCodecPackage">
		<rdfs:subClassOf rdf:resource="&java;JavaAPIPart"/>
		<rdfs:seeAlso rdf:resource="#OrgOmgCORBAPortable"/>
		<rdfs:seeAlso rdf:resource="#JavaLang"/>
		<rdfs:seeAlso rdf:resource="#OrgOmgCORBA"/>
		<rdfs:comment xml:lang="en">Java API part implementing the org.omg.IOP.CodecPackage package for J2SE 1.4</rdfs:comment>
	</owl:Class>
	<owl:Class rdf:about="#OrgOmgMessaging">
		<rdfs:subClassOf rdf:resource="&java;JavaAPIPart"/>
		<rdfs:seeAlso rdf:resource="#OrgOmgCORBAPortable"/>
		<rdfs:seeAlso rdf:resource="#JavaLang"/>
		<rdfs:seeAlso rdf:resource="#OrgOmgCORBA"/>
		<rdfs:comment xml:lang="en">Java API part implementing the org.omg.Messaging package for J2SE 1.4</rdfs:comment>
	</owl:Class>
	<owl:Class rdf:about="#OrgOmgPortableInterceptor">
		<rdfs:subClassOf rdf:resource="&java;JavaAPIPart"/>
		<rdfs:seeAlso rdf:resource="#OrgOmgCORBA"/>
		<rdfs:seeAlso rdf:resource="#OrgOmgIOP"/>
		<rdfs:seeAlso rdf:resource="#OrgOmgCORBAPortable"/>
		<rdfs:seeAlso rdf:resource="#JavaLang"/>
		<rdfs:comment xml:lang="en">Java API part implementing the org.omg.PortableInterceptor package for J2SE 1.4</rdfs:comment>
	</owl:Class>
	<owl:Class rdf:about="#OrgOmgPortableInterceptorORBInitInfoPackage">
		<rdfs:subClassOf rdf:resource="&java;JavaAPIPart"/>
		<rdfs:seeAlso rdf:resource="#OrgOmgCORBAPortable"/>
		<rdfs:seeAlso rdf:resource="#JavaLang"/>
		<rdfs:seeAlso rdf:resource="#OrgOmgCORBA"/>
		<rdfs:comment xml:lang="en">Java API part implementing the org.omg.PortableInterceptor.ORBInitInfoPackage package for J2SE 1.4</rdfs:comment>
	</owl:Class>
	<owl:Class rdf:about="#OrgOmgStubJavaRmi">
		<owl:equivalentClass rdf:resource="&j2se-1_3;OrgOmgStubJavaRmi"/>
		<rdfs:subClassOf rdf:resource="&java;JavaAPIPart"/>
		<rdfs:seeAlso rdf:resource="#JavaRmi"/>
		<rdfs:seeAlso rdf:resource="#JavaxRmiCORBA"/>
		<rdfs:comment xml:lang="en">Java API part implementing the org.omg.stub.java.rmi package for J2SE 1.4</rdfs:comment>
	</owl:Class>
	<owl:Class rdf:about="#OrgXmlSax">
		<rdfs:subClassOf rdf:resource="&java;JavaAPIPart"/>
		<rdfs:seeAlso rdf:resource="#JavaUtil"/>
		<rdfs:seeAlso rdf:resource="#JavaLang"/>
		<rdfs:seeAlso rdf:resource="#JavaIo"/>
		<rdfs:comment xml:lang="en">Java API part implementing the org.xml.sax package for J2SE 1.4</rdfs:comment>
	</owl:Class>
	<owl:Class rdf:about="#OrgXmlSaxHelpers">
		<rdfs:subClassOf rdf:resource="&java;JavaAPIPart"/>
		<rdfs:seeAlso rdf:resource="#OrgXmlSax"/>
		<rdfs:seeAlso rdf:resource="#JavaUtil"/>
		<rdfs:seeAlso rdf:resource="#JavaLang"/>
		<rdfs:comment xml:lang="en">Java API part implementing the org.xml.sax.helpers package for J2SE 1.4</rdfs:comment>
	</owl:Class>
	<owl:Class rdf:about="#OrgXmlSaxExt">
		<rdfs:subClassOf rdf:resource="&java;JavaAPIPart"/>
		<rdfs:seeAlso rdf:resource="#JavaLang"/>
		<rdfs:comment xml:lang="en">Java API part implementing the org.xml.sax.ext package for J2SE 1.4</rdfs:comment>
	</owl:Class>
	<owl:Class rdf:about="#OrgIetfJgss">
		<rdfs:subClassOf rdf:resource="&java;JavaAPIPart"/>
		<rdfs:seeAlso rdf:resource="#JavaNet"/>
		<rdfs:seeAlso rdf:resource="#JavaSecurity"/>
		<rdfs:seeAlso rdf:resource="#JavaLang"/>
		<rdfs:seeAlso rdf:resource="#JavaIo"/>
		<rdfs:comment xml:lang="en">Java API part implementing the org.ietf.jgss package for J2SE 1.4</rdfs:comment>
	</owl:Class>
	<owl:Class rdf:about="#JavaLangAPI">
		<rdfs:subClassOf rdf:resource="&j2me-pp-1_1;JavaLangAPI"/>
		<rdfs:subClassOf rdf:resource="&j2se-1_3;JavaLangAPI"/>
		<rdfs:comment xml:lang="en">JavaLibrary implementing the java.lang package for J2SE 1.4</rdfs:comment>
		<rdfs:comment xml:lang="OWLManchester">platform:comprisesInterfacePart some JavaLang</rdfs:comment>
	</owl:Class>
	<owl:Class rdf:about="#JavaLangReflectAPI">
		<owl:equivalentClass rdf:resource="&j2me-pp-1_1;JavaLangReflectAPI"/>
		<rdfs:subClassOf rdf:resource="&j2se-1_3;JavaLangReflectAPI"/>
		<rdfs:comment xml:lang="en">JavaLibrary implementing the java.lang.reflect package for J2SE 1.4</rdfs:comment>
		<rdfs:comment xml:lang="OWLManchester">platform:comprisesInterfacePart some JavaLangReflect</rdfs:comment>
	</owl:Class>
	<owl:Class rdf:about="#JavaLangRefAPI">
		<owl:equivalentClass rdf:resource="&j2me-pp-1_1;JavaLangRefAPI"/>
		<owl:equivalentClass rdf:resource="&j2se-1_3;JavaLangRefAPI"/>
		<rdfs:subClassOf rdf:resource="&java;JavaAPI"/>
		<rdfs:comment xml:lang="en">JavaLibrary implementing the java.lang.ref package for J2SE 1.4</rdfs:comment>
		<rdfs:comment xml:lang="OWLManchester">platform:comprisesInterfacePart some JavaLangRef</rdfs:comment>
	</owl:Class>
	<owl:Class rdf:about="#JavaIoAPI">
		<rdfs:subClassOf rdf:resource="&j2me-pp-1_1;JavaIoAPI"/>
		<rdfs:subClassOf rdf:resource="&j2se-1_3;JavaIoAPI"/>
		<rdfs:comment xml:lang="en">JavaLibrary implementing the java.io package for J2SE 1.4</rdfs:comment>
		<rdfs:comment xml:lang="OWLManchester">platform:comprisesInterfacePart some JavaIo</rdfs:comment>
	</owl:Class>
	<owl:Class rdf:about="#JavaUtilAPI">
		<rdfs:subClassOf rdf:resource="&j2me-pp-1_1;JavaUtilAPI"/>
		<rdfs:subClassOf rdf:resource="&j2se-1_3;JavaUtilAPI"/>
		<rdfs:comment xml:lang="en">JavaLibrary implementing the java.util package for J2SE 1.4</rdfs:comment>
		<rdfs:comment xml:lang="OWLManchester">platform:comprisesInterfacePart some JavaUtil</rdfs:comment>
	</owl:Class>
	<owl:Class rdf:about="#JavaUtilLoggingAPI">
		<rdfs:subClassOf rdf:resource="&java;JavaAPI"/>
		<rdfs:comment xml:lang="en">JavaLibrary implementing the java.util.logging package for J2SE 1.4</rdfs:comment>
		<rdfs:comment xml:lang="OWLManchester">platform:comprisesInterfacePart some JavaUtilLogging</rdfs:comment>
	</owl:Class>
	<owl:Class rdf:about="#JavaUtilJarAPI">
		<owl:equivalentClass rdf:resource="&j2me-pp-1_1;JavaUtilJarAPI"/>
		<rdfs:subClassOf rdf:resource="&j2se-1_3;JavaUtilJarAPI"/>
		<rdfs:comment xml:lang="en">JavaLibrary implementing the java.util.jar package for J2SE 1.4</rdfs:comment>
		<rdfs:comment xml:lang="OWLManchester">platform:comprisesInterfacePart some JavaUtilJar</rdfs:comment>
	</owl:Class>
	<owl:Class rdf:about="#JavaUtilZipAPI">
		<owl:equivalentClass rdf:resource="&j2me-pp-1_1;JavaUtilZipAPI"/>
		<rdfs:subClassOf rdf:resource="&j2se-1_3;JavaUtilZipAPI"/>
		<rdfs:comment xml:lang="en">JavaLibrary implementing the java.util.zip package for J2SE 1.4</rdfs:comment>
		<rdfs:comment xml:lang="OWLManchester">platform:comprisesInterfacePart some JavaUtilZip</rdfs:comment>
	</owl:Class>
	<owl:Class rdf:about="#JavaUtilPrefsAPI">
		<rdfs:subClassOf rdf:resource="&java;JavaAPI"/>
		<rdfs:comment xml:lang="en">JavaLibrary implementing the java.util.prefs package for J2SE 1.4</rdfs:comment>
		<rdfs:comment xml:lang="OWLManchester">platform:comprisesInterfacePart some JavaUtilPrefs</rdfs:comment>
	</owl:Class>
	<owl:Class rdf:about="#JavaUtilRegexAPI">
		<rdfs:subClassOf rdf:resource="&java;JavaAPI"/>
		<rdfs:comment xml:lang="en">JavaLibrary implementing the java.util.regex package for J2SE 1.4</rdfs:comment>
		<rdfs:comment xml:lang="OWLManchester">platform:comprisesInterfacePart some JavaUtilRegex</rdfs:comment>
	</owl:Class>
	<owl:Class rdf:about="#JavaNetAPI">
		<rdfs:subClassOf rdf:resource="&j2me-pp-1_1;JavaNetAPI"/>
		<rdfs:subClassOf rdf:resource="&j2se-1_3;JavaNetAPI"/>
		<rdfs:comment xml:lang="en">JavaLibrary implementing the java.net package for J2SE 1.4</rdfs:comment>
		<rdfs:comment xml:lang="OWLManchester">platform:comprisesInterfacePart some JavaNet</rdfs:comment>
	</owl:Class>
	<owl:Class rdf:about="#JavaSecurityAPI">
		<rdfs:subClassOf rdf:resource="&j2me-pp-1_1;JavaSecurityAPI"/>
		<rdfs:subClassOf rdf:resource="&j2se-1_3;JavaSecurityAPI"/>
		<rdfs:comment xml:lang="en">JavaLibrary implementing the java.security package for J2SE 1.4</rdfs:comment>
		<rdfs:comment xml:lang="OWLManchester">platform:comprisesInterfacePart some JavaSecurity</rdfs:comment>
	</owl:Class>
	<owl:Class rdf:about="#JavaSecurityCertAPI">
		<rdfs:subClassOf rdf:resource="&j2me-pp-1_1;JavaSecurityCertAPI"/>
		<rdfs:subClassOf rdf:resource="&j2se-1_3;JavaSecurityCertAPI"/>
		<rdfs:comment xml:lang="en">JavaLibrary implementing the java.security.cert package for J2SE 1.4</rdfs:comment>
		<rdfs:comment xml:lang="OWLManchester">platform:comprisesInterfacePart some JavaSecurityCert</rdfs:comment>
	</owl:Class>
	<owl:Class rdf:about="#JavaSecuritySpecAPI">
		<rdfs:subClassOf rdf:resource="&j2me-pp-1_1;JavaSecuritySpecAPI"/>
		<rdfs:subClassOf rdf:resource="&j2se-1_3;JavaSecuritySpecAPI"/>
		<rdfs:comment xml:lang="en">JavaLibrary implementing the java.security.spec package for J2SE 1.4</rdfs:comment>
		<rdfs:comment xml:lang="OWLManchester">platform:comprisesInterfacePart some JavaSecuritySpec</rdfs:comment>
	</owl:Class>
	<owl:Class rdf:about="#JavaSecurityAclAPI">
		<owl:equivalentClass rdf:resource="&j2me-pp-1_1;JavaSecurityAclAPI"/>
		<rdfs:subClassOf rdf:resource="&j2se-1_3;JavaSecurityAclAPI"/>
		<rdfs:comment xml:lang="en">JavaLibrary implementing the java.security.acl package for J2SE 1.4</rdfs:comment>
		<rdfs:comment xml:lang="OWLManchester">platform:comprisesInterfacePart some JavaSecurityAcl</rdfs:comment>
	</owl:Class>
	<owl:Class rdf:about="#JavaSecurityInterfacesAPI">
		<rdfs:subClassOf rdf:resource="&j2me-pp-1_1;JavaSecurityInterfacesAPI"/>
		<rdfs:subClassOf rdf:resource="&j2se-1_3;JavaSecurityInterfacesAPI"/>
		<rdfs:comment xml:lang="en">JavaLibrary implementing the java.security.interfaces package for J2SE 1.4</rdfs:comment>
		<rdfs:comment xml:lang="OWLManchester">platform:comprisesInterfacePart some JavaSecurityInterfaces</rdfs:comment>
	</owl:Class>
	<owl:Class rdf:about="#JavaNioAPI">
		<rdfs:subClassOf rdf:resource="&java;JavaAPI"/>
		<rdfs:comment xml:lang="en">JavaLibrary implementing the java.nio package for J2SE 1.4</rdfs:comment>
		<rdfs:comment xml:lang="OWLManchester">platform:comprisesInterfacePart some JavaNio</rdfs:comment>
	</owl:Class>
	<owl:Class rdf:about="#JavaNioChannelsAPI">
		<rdfs:subClassOf rdf:resource="&java;JavaAPI"/>
		<rdfs:comment xml:lang="en">JavaLibrary implementing the java.nio.channels package for J2SE 1.4</rdfs:comment>
		<rdfs:comment xml:lang="OWLManchester">platform:comprisesInterfacePart some JavaNioChannels</rdfs:comment>
	</owl:Class>
	<owl:Class rdf:about="#JavaNioChannelsSpiAPI">
		<rdfs:subClassOf rdf:resource="&java;JavaAPI"/>
		<rdfs:comment xml:lang="en">JavaLibrary implementing the java.nio.channels.spi package for J2SE 1.4</rdfs:comment>
		<rdfs:comment xml:lang="OWLManchester">platform:comprisesInterfacePart some JavaNioChannelsSpi</rdfs:comment>
	</owl:Class>
	<owl:Class rdf:about="#JavaNioCharsetAPI">
		<rdfs:subClassOf rdf:resource="&java;JavaAPI"/>
		<rdfs:comment xml:lang="en">JavaLibrary implementing the java.nio.charset package for J2SE 1.4</rdfs:comment>
		<rdfs:comment xml:lang="OWLManchester">platform:comprisesInterfacePart some JavaNioCharset</rdfs:comment>
	</owl:Class>
	<owl:Class rdf:about="#JavaNioCharsetSpiAPI">
		<rdfs:subClassOf rdf:resource="&java;JavaAPI"/>
		<rdfs:comment xml:lang="en">JavaLibrary implementing the java.nio.charset.spi package for J2SE 1.4</rdfs:comment>
		<rdfs:comment xml:lang="OWLManchester">platform:comprisesInterfacePart some JavaNioCharsetSpi</rdfs:comment>
	</owl:Class>
	<owl:Class rdf:about="#JavaBeansAPI">
		<rdfs:subClassOf rdf:resource="&j2me-pp-1_1;JavaBeansAPI"/>
		<rdfs:subClassOf rdf:resource="&j2se-1_3;JavaBeansAPI"/>
		<rdfs:comment xml:lang="en">JavaLibrary implementing the java.beans package for J2SE 1.4</rdfs:comment>
		<rdfs:comment xml:lang="OWLManchester">platform:comprisesInterfacePart some JavaBeans</rdfs:comment>
	</owl:Class>
	<owl:Class rdf:about="#JavaBeansBeancontextAPI">
		<owl:equivalentClass rdf:resource="&j2se-1_3;JavaBeansBeancontextAPI"/>
		<rdfs:subClassOf rdf:resource="&java;JavaAPI"/>
		<rdfs:comment xml:lang="en">JavaLibrary implementing the java.beans.beancontext package for J2SE 1.4</rdfs:comment>
		<rdfs:comment xml:lang="OWLManchester">platform:comprisesInterfacePart some JavaBeansBeancontext</rdfs:comment>
	</owl:Class>
	<owl:Class rdf:about="#JavaAwtAPI">
		<rdfs:subClassOf rdf:resource="&j2me-pp-1_1;JavaAwtAPI"/>
		<rdfs:subClassOf rdf:resource="&j2se-1_3;JavaAwtAPI"/>
		<rdfs:comment xml:lang="en">JavaLibrary implementing the java.awt package for J2SE 1.4</rdfs:comment>
		<rdfs:comment xml:lang="OWLManchester">platform:comprisesInterfacePart some JavaAwt</rdfs:comment>
	</owl:Class>
	<owl:Class rdf:about="#JavaAwtImageAPI">
		<rdfs:subClassOf rdf:resource="&j2me-pp-1_1;JavaAwtImageAPI"/>
		<rdfs:subClassOf rdf:resource="&j2se-1_3;JavaAwtImageAPI"/>
		<rdfs:comment xml:lang="en">JavaLibrary implementing the java.awt.image package for J2SE 1.4</rdfs:comment>
		<rdfs:comment xml:lang="OWLManchester">platform:comprisesInterfacePart some JavaAwtImage</rdfs:comment>
	</owl:Class>
	<owl:Class rdf:about="#JavaAwtImageRenderableAPI">
		<owl:equivalentClass rdf:resource="&j2se-1_3;JavaAwtImageRenderableAPI"/>
		<rdfs:subClassOf rdf:resource="&java;JavaAPI"/>
		<rdfs:comment xml:lang="en">JavaLibrary implementing the java.awt.image.renderable package for J2SE 1.4</rdfs:comment>
		<rdfs:comment xml:lang="OWLManchester">platform:comprisesInterfacePart some JavaAwtImageRenderable</rdfs:comment>
	</owl:Class>
	<owl:Class rdf:about="#JavaAwtDatatransferAPI">
		<rdfs:subClassOf rdf:resource="&j2me-pp-1_1;JavaAwtDatatransferAPI"/>
		<rdfs:subClassOf rdf:resource="&j2se-1_3;JavaAwtDatatransferAPI"/>
		<rdfs:comment xml:lang="en">JavaLibrary implementing the java.awt.datatransfer package for J2SE 1.4</rdfs:comment>
		<rdfs:comment xml:lang="OWLManchester">platform:comprisesInterfacePart some JavaAwtDatatransfer</rdfs:comment>
	</owl:Class>
	<owl:Class rdf:about="#JavaAwtDndAPI">
		<rdfs:subClassOf rdf:resource="&j2se-1_3;JavaAwtDndAPI"/>
		<rdfs:comment xml:lang="en">JavaLibrary implementing the java.awt.dnd package for J2SE 1.4</rdfs:comment>
		<rdfs:comment xml:lang="OWLManchester">platform:comprisesInterfacePart some JavaAwtDnd</rdfs:comment>
	</owl:Class>
	<owl:Class rdf:about="#JavaAwtEventAPI">
		<rdfs:subClassOf rdf:resource="&j2me-pp-1_1;JavaAwtEventAPI"/>
		<rdfs:subClassOf rdf:resource="&j2se-1_3;JavaAwtEventAPI"/>
		<rdfs:comment xml:lang="en">JavaLibrary implementing the java.awt.event package for J2SE 1.4</rdfs:comment>
		<rdfs:comment xml:lang="OWLManchester">platform:comprisesInterfacePart some JavaAwtEvent</rdfs:comment>
	</owl:Class>
	<owl:Class rdf:about="#JavaAwtImAPI">
		<owl:equivalentClass rdf:resource="&j2se-1_3;JavaAwtImAPI"/>
		<rdfs:subClassOf rdf:resource="&j2me-pp-1_1;JavaAwtImAPI"/>
		<rdfs:comment xml:lang="en">JavaLibrary implementing the java.awt.im package for J2SE 1.4</rdfs:comment>
		<rdfs:comment xml:lang="OWLManchester">platform:comprisesInterfacePart some JavaAwtIm</rdfs:comment>
	</owl:Class>
	<owl:Class rdf:about="#JavaAwtImSpiAPI">
		<rdfs:subClassOf rdf:resource="&j2se-1_3;JavaAwtImSpiAPI"/>
		<rdfs:comment xml:lang="en">JavaLibrary implementing the java.awt.im.spi package for J2SE 1.4</rdfs:comment>
		<rdfs:comment xml:lang="OWLManchester">platform:comprisesInterfacePart some JavaAwtImSpi</rdfs:comment>
	</owl:Class>
	<owl:Class rdf:about="#JavaAwtFontAPI">
		<rdfs:subClassOf rdf:resource="&j2me-pp-1_1;JavaAwtFontAPI"/>
		<rdfs:subClassOf rdf:resource="&j2se-1_3;JavaAwtFontAPI"/>
		<rdfs:comment xml:lang="en">JavaLibrary implementing the java.awt.font package for J2SE 1.4</rdfs:comment>
		<rdfs:comment xml:lang="OWLManchester">platform:comprisesInterfacePart some JavaAwtFont</rdfs:comment>
	</owl:Class>
	<owl:Class rdf:about="#JavaAwtGeomAPI">
		<rdfs:subClassOf rdf:resource="&j2se-1_3;JavaAwtGeomAPI"/>
		<rdfs:comment xml:lang="en">JavaLibrary implementing the java.awt.geom package for J2SE 1.4</rdfs:comment>
		<rdfs:comment xml:lang="OWLManchester">platform:comprisesInterfacePart some JavaAwtGeom</rdfs:comment>
	</owl:Class>
	<owl:Class rdf:about="#JavaAwtColorAPI">
		<rdfs:subClassOf rdf:resource="&j2me-pp-1_1;JavaAwtColorAPI"/>
		<rdfs:subClassOf rdf:resource="&j2se-1_3;JavaAwtColorAPI"/>
		<rdfs:comment xml:lang="en">JavaLibrary implementing the java.awt.color package for J2SE 1.4</rdfs:comment>
		<rdfs:comment xml:lang="OWLManchester">platform:comprisesInterfacePart some JavaAwtColor</rdfs:comment>
	</owl:Class>
	<owl:Class rdf:about="#JavaAwtPrintAPI">
		<rdfs:subClassOf rdf:resource="&j2se-1_3;JavaAwtPrintAPI"/>
		<rdfs:comment xml:lang="en">JavaLibrary implementing the java.awt.print package for J2SE 1.4</rdfs:comment>
		<rdfs:comment xml:lang="OWLManchester">platform:comprisesInterfacePart some JavaAwtPrint</rdfs:comment>
	</owl:Class>
	<owl:Class rdf:about="#JavaTextAPI">
		<rdfs:subClassOf rdf:resource="&j2se-1_3;JavaTextAPI"/>
		<rdfs:comment xml:lang="en">JavaLibrary implementing the java.text package for J2SE 1.4</rdfs:comment>
		<rdfs:comment xml:lang="OWLManchester">platform:comprisesInterfacePart some JavaText</rdfs:comment>
	</owl:Class>
	<owl:Class rdf:about="#JavaMathAPI">
		<rdfs:subClassOf rdf:resource="&j2me-pp-1_1;JavaMathAPI"/>
		<rdfs:subClassOf rdf:resource="&j2se-1_3;JavaMathAPI"/>
		<rdfs:comment xml:lang="en">JavaLibrary implementing the java.math package for J2SE 1.4</rdfs:comment>
		<rdfs:comment xml:lang="OWLManchester">platform:comprisesInterfacePart some JavaMath</rdfs:comment>
	</owl:Class>
	<owl:Class rdf:about="#JavaAppletAPI">
		<rdfs:subClassOf rdf:resource="&j2me-pp-1_1;JavaAppletAPI"/>
		<rdfs:subClassOf rdf:resource="&j2se-1_3;JavaAppletAPI"/>
		<rdfs:comment xml:lang="en">JavaLibrary implementing the java.applet package for J2SE 1.4</rdfs:comment>
		<rdfs:comment xml:lang="OWLManchester">platform:comprisesInterfacePart some JavaApplet</rdfs:comment>
	</owl:Class>
	<owl:Class rdf:about="#JavaRmiAPI">
		<rdfs:subClassOf rdf:resource="&j2me-pp-1_1;JavaRmiAPI"/>
		<rdfs:subClassOf rdf:resource="&j2se-1_3;JavaRmiAPI"/>
		<rdfs:comment xml:lang="en">JavaLibrary implementing the java.rmi package for J2SE 1.4</rdfs:comment>
		<rdfs:comment xml:lang="OWLManchester">platform:comprisesInterfacePart some JavaRmi</rdfs:comment>
	</owl:Class>
	<owl:Class rdf:about="#JavaRmiActivationAPI">
		<rdfs:subClassOf rdf:resource="&j2se-1_3;JavaRmiActivationAPI"/>
		<rdfs:comment xml:lang="en">JavaLibrary implementing the java.rmi.activation package for J2SE 1.4</rdfs:comment>
		<rdfs:comment xml:lang="OWLManchester">platform:comprisesInterfacePart some JavaRmiActivation</rdfs:comment>
	</owl:Class>
	<owl:Class rdf:about="#JavaRmiServerAPI">
		<rdfs:subClassOf rdf:resource="&j2se-1_3;JavaRmiServerAPI"/>
		<rdfs:comment xml:lang="en">JavaLibrary implementing the java.rmi.server package for J2SE 1.4</rdfs:comment>
		<rdfs:comment xml:lang="OWLManchester">platform:comprisesInterfacePart some JavaRmiServer</rdfs:comment>
	</owl:Class>
	<owl:Class rdf:about="#JavaRmiDgcAPI">
		<owl:equivalentClass rdf:resource="&j2se-1_3;JavaRmiDgcAPI"/>
		<rdfs:subClassOf rdf:resource="&java;JavaAPI"/>
		<rdfs:comment xml:lang="en">JavaLibrary implementing the java.rmi.dgc package for J2SE 1.4</rdfs:comment>
		<rdfs:comment xml:lang="OWLManchester">platform:comprisesInterfacePart some JavaRmiDgc</rdfs:comment>
	</owl:Class>
	<owl:Class rdf:about="#JavaRmiRegistryAPI">
		<owl:equivalentClass rdf:resource="&j2se-1_3;JavaRmiRegistryAPI"/>
		<rdfs:subClassOf rdf:resource="&j2me-pp-1_1;JavaRmiRegistryAPI"/>
		<rdfs:comment xml:lang="en">JavaLibrary implementing the java.rmi.registry package for J2SE 1.4</rdfs:comment>
		<rdfs:comment xml:lang="OWLManchester">platform:comprisesInterfacePart some JavaRmiRegistry</rdfs:comment>
	</owl:Class>
	<owl:Class rdf:about="#JavaSqlAPI">
		<rdfs:subClassOf rdf:resource="&j2se-1_3;JavaSqlAPI"/>
		<rdfs:comment xml:lang="en">JavaLibrary implementing the java.sql package for J2SE 1.4</rdfs:comment>
		<rdfs:comment xml:lang="OWLManchester">platform:comprisesInterfacePart some JavaSql</rdfs:comment>
	</owl:Class>
	<owl:Class rdf:about="#JavaxImageioAPI">
		<rdfs:subClassOf rdf:resource="&java;JavaAPI"/>
		<rdfs:comment xml:lang="en">JavaLibrary implementing the javax.imageio package for J2SE 1.4</rdfs:comment>
		<rdfs:comment xml:lang="OWLManchester">platform:comprisesInterfacePart some JavaxImageio</rdfs:comment>
	</owl:Class>
	<owl:Class rdf:about="#JavaxImageioSpiAPI">
		<rdfs:subClassOf rdf:resource="&java;JavaAPI"/>
		<rdfs:comment xml:lang="en">JavaLibrary implementing the javax.imageio.spi package for J2SE 1.4</rdfs:comment>
		<rdfs:comment xml:lang="OWLManchester">platform:comprisesInterfacePart some JavaxImageioSpi</rdfs:comment>
	</owl:Class>
	<owl:Class rdf:about="#JavaxImageioMetadataAPI">
		<rdfs:subClassOf rdf:resource="&java;JavaAPI"/>
		<rdfs:comment xml:lang="en">JavaLibrary implementing the javax.imageio.metadata package for J2SE 1.4</rdfs:comment>
		<rdfs:comment xml:lang="OWLManchester">platform:comprisesInterfacePart some JavaxImageioMetadata</rdfs:comment>
	</owl:Class>
	<owl:Class rdf:about="#JavaxImageioStreamAPI">
		<rdfs:subClassOf rdf:resource="&java;JavaAPI"/>
		<rdfs:comment xml:lang="en">JavaLibrary implementing the javax.imageio.stream package for J2SE 1.4</rdfs:comment>
		<rdfs:comment xml:lang="OWLManchester">platform:comprisesInterfacePart some JavaxImageioStream</rdfs:comment>
	</owl:Class>
	<owl:Class rdf:about="#JavaxImageioEventAPI">
		<rdfs:subClassOf rdf:resource="&java;JavaAPI"/>
		<rdfs:comment xml:lang="en">JavaLibrary implementing the javax.imageio.event package for J2SE 1.4</rdfs:comment>
		<rdfs:comment xml:lang="OWLManchester">platform:comprisesInterfacePart some JavaxImageioEvent</rdfs:comment>
	</owl:Class>
	<owl:Class rdf:about="#JavaxImageioPluginsJpegAPI">
		<rdfs:subClassOf rdf:resource="&java;JavaAPI"/>
		<rdfs:comment xml:lang="en">JavaLibrary implementing the javax.imageio.plugins.jpeg package for J2SE 1.4</rdfs:comment>
		<rdfs:comment xml:lang="OWLManchester">platform:comprisesInterfacePart some JavaxImageioPluginsJpeg</rdfs:comment>
	</owl:Class>
	<owl:Class rdf:about="#JavaxAccessibilityAPI">
		<rdfs:subClassOf rdf:resource="&j2se-1_3;JavaxAccessibilityAPI"/>
		<rdfs:comment xml:lang="en">JavaLibrary implementing the javax.accessibility package for J2SE 1.4</rdfs:comment>
		<rdfs:comment xml:lang="OWLManchester">platform:comprisesInterfacePart some JavaxAccessibility</rdfs:comment>
	</owl:Class>
	<owl:Class rdf:about="#JavaxSwingAPI">
		<rdfs:subClassOf rdf:resource="&java;JavaAPI"/>
		<rdfs:comment xml:lang="en">JavaLibrary implementing the javax.swing package for J2SE 1.4</rdfs:comment>
		<rdfs:comment xml:lang="OWLManchester">platform:comprisesInterfacePart some JavaxSwing</rdfs:comment>
	</owl:Class>
	<owl:Class rdf:about="#JavaxSwingPlafAPI">
		<rdfs:subClassOf rdf:resource="&j2se-1_3;JavaxSwingPlafAPI"/>
		<rdfs:comment xml:lang="en">JavaLibrary implementing the javax.swing.plaf package for J2SE 1.4</rdfs:comment>
		<rdfs:comment xml:lang="OWLManchester">platform:comprisesInterfacePart some JavaxSwingPlaf</rdfs:comment>
	</owl:Class>
	<owl:Class rdf:about="#JavaxSwingPlafBasicAPI">
		<rdfs:subClassOf rdf:resource="&j2se-1_3;JavaxSwingPlafBasicAPI"/>
		<rdfs:comment xml:lang="en">JavaLibrary implementing the javax.swing.plaf.basic package for J2SE 1.4</rdfs:comment>
		<rdfs:comment xml:lang="OWLManchester">platform:comprisesInterfacePart some JavaxSwingPlafBasic</rdfs:comment>
	</owl:Class>
	<owl:Class rdf:about="#JavaxSwingPlafMetalAPI">
		<rdfs:subClassOf rdf:resource="&j2se-1_3;JavaxSwingPlafMetalAPI"/>
		<rdfs:comment xml:lang="en">JavaLibrary implementing the javax.swing.plaf.metal package for J2SE 1.4</rdfs:comment>
		<rdfs:comment xml:lang="OWLManchester">platform:comprisesInterfacePart some JavaxSwingPlafMetal</rdfs:comment>
	</owl:Class>
	<owl:Class rdf:about="#JavaxSwingPlafMultiAPI">
		<rdfs:subClassOf rdf:resource="&j2se-1_3;JavaxSwingPlafMultiAPI"/>
		<rdfs:comment xml:lang="en">JavaLibrary implementing the javax.swing.plaf.multi package for J2SE 1.4</rdfs:comment>
		<rdfs:comment xml:lang="OWLManchester">platform:comprisesInterfacePart some JavaxSwingPlafMulti</rdfs:comment>
	</owl:Class>
	<owl:Class rdf:about="#JavaxSwingEventAPI">
		<rdfs:subClassOf rdf:resource="&j2se-1_3;JavaxSwingEventAPI"/>
		<rdfs:comment xml:lang="en">JavaLibrary implementing the javax.swing.event package for J2SE 1.4</rdfs:comment>
		<rdfs:comment xml:lang="OWLManchester">platform:comprisesInterfacePart some JavaxSwingEvent</rdfs:comment>
	</owl:Class>
	<owl:Class rdf:about="#JavaxSwingBorderAPI">
		<owl:equivalentClass rdf:resource="&j2se-1_3;JavaxSwingBorderAPI"/>
		<rdfs:subClassOf rdf:resource="&java;JavaAPI"/>
		<rdfs:comment xml:lang="en">JavaLibrary implementing the javax.swing.border package for J2SE 1.4</rdfs:comment>
		<rdfs:comment xml:lang="OWLManchester">platform:comprisesInterfacePart some JavaxSwingBorder</rdfs:comment>
	</owl:Class>
	<owl:Class rdf:about="#JavaxSwingTextAPI">
		<rdfs:subClassOf rdf:resource="&j2se-1_3;JavaxSwingTextAPI"/>
		<rdfs:comment xml:lang="en">JavaLibrary implementing the javax.swing.text package for J2SE 1.4</rdfs:comment>
		<rdfs:comment xml:lang="OWLManchester">platform:comprisesInterfacePart some JavaxSwingText</rdfs:comment>
	</owl:Class>
	<owl:Class rdf:about="#JavaxSwingTextHtmlAPI">
		<rdfs:subClassOf rdf:resource="&j2se-1_3;JavaxSwingTextHtmlAPI"/>
		<rdfs:comment xml:lang="en">JavaLibrary implementing the javax.swing.text.html package for J2SE 1.4</rdfs:comment>
		<rdfs:comment xml:lang="OWLManchester">platform:comprisesInterfacePart some JavaxSwingTextHtml</rdfs:comment>
	</owl:Class>
	<owl:Class rdf:about="#JavaxSwingTextHtmlParserAPI">
		<owl:equivalentClass rdf:resource="&j2se-1_3;JavaxSwingTextHtmlParserAPI"/>
		<rdfs:subClassOf rdf:resource="&java;JavaAPI"/>
		<rdfs:comment xml:lang="en">JavaLibrary implementing the javax.swing.text.html.parser package for J2SE 1.4</rdfs:comment>
		<rdfs:comment xml:lang="OWLManchester">platform:comprisesInterfacePart some JavaxSwingTextHtmlParser</rdfs:comment>
	</owl:Class>
	<owl:Class rdf:about="#JavaxSwingTextRtfAPI">
		<owl:equivalentClass rdf:resource="&j2se-1_3;JavaxSwingTextRtfAPI"/>
		<rdfs:subClassOf rdf:resource="&java;JavaAPI"/>
		<rdfs:comment xml:lang="en">JavaLibrary implementing the javax.swing.text.rtf package for J2SE 1.4</rdfs:comment>
		<rdfs:comment xml:lang="OWLManchester">platform:comprisesInterfacePart some JavaxSwingTextRtf</rdfs:comment>
	</owl:Class>
	<owl:Class rdf:about="#JavaxSwingTableAPI">
		<rdfs:subClassOf rdf:resource="&j2se-1_3;JavaxSwingTableAPI"/>
		<rdfs:comment xml:lang="en">JavaLibrary implementing the javax.swing.table package for J2SE 1.4</rdfs:comment>
		<rdfs:comment xml:lang="OWLManchester">platform:comprisesInterfacePart some JavaxSwingTable</rdfs:comment>
	</owl:Class>
	<owl:Class rdf:about="#JavaxSwingUndoAPI">
		<rdfs:subClassOf rdf:resource="&j2se-1_3;JavaxSwingUndoAPI"/>
		<rdfs:comment xml:lang="en">JavaLibrary implementing the javax.swing.undo package for J2SE 1.4</rdfs:comment>
		<rdfs:comment xml:lang="OWLManchester">platform:comprisesInterfacePart some JavaxSwingUndo</rdfs:comment>
	</owl:Class>
	<owl:Class rdf:about="#JavaxSwingTreeAPI">
		<rdfs:subClassOf rdf:resource="&j2se-1_3;JavaxSwingTreeAPI"/>
		<rdfs:comment xml:lang="en">JavaLibrary implementing the javax.swing.tree package for J2SE 1.4</rdfs:comment>
		<rdfs:comment xml:lang="OWLManchester">platform:comprisesInterfacePart some JavaxSwingTree</rdfs:comment>
	</owl:Class>
	<owl:Class rdf:about="#JavaxSwingFilechooserAPI">
		<rdfs:subClassOf rdf:resource="&j2se-1_3;JavaxSwingFilechooserAPI"/>
		<rdfs:comment xml:lang="en">JavaLibrary implementing the javax.swing.filechooser package for J2SE 1.4</rdfs:comment>
		<rdfs:comment xml:lang="OWLManchester">platform:comprisesInterfacePart some JavaxSwingFilechooser</rdfs:comment>
	</owl:Class>
	<owl:Class rdf:about="#JavaxSwingColorchooserAPI">
		<rdfs:subClassOf rdf:resource="&j2se-1_3;JavaxSwingColorchooserAPI"/>
		<rdfs:comment xml:lang="en">JavaLibrary implementing the javax.swing.colorchooser package for J2SE 1.4</rdfs:comment>
		<rdfs:comment xml:lang="OWLManchester">platform:comprisesInterfacePart some JavaxSwingColorchooser</rdfs:comment>
	</owl:Class>
	<owl:Class rdf:about="#JavaxSoundSampledAPI">
		<rdfs:subClassOf rdf:resource="&j2se-1_3;JavaxSoundSampledAPI"/>
		<rdfs:comment xml:lang="en">JavaLibrary implementing the javax.sound.sampled package for J2SE 1.4</rdfs:comment>
		<rdfs:comment xml:lang="OWLManchester">platform:comprisesInterfacePart some JavaxSoundSampled</rdfs:comment>
	</owl:Class>
	<owl:Class rdf:about="#JavaxSoundSampledSpiAPI">
		<owl:equivalentClass rdf:resource="&j2se-1_3;JavaxSoundSampledSpiAPI"/>
		<rdfs:subClassOf rdf:resource="&java;JavaAPI"/>
		<rdfs:comment xml:lang="en">JavaLibrary implementing the javax.sound.sampled.spi package for J2SE 1.4</rdfs:comment>
		<rdfs:comment xml:lang="OWLManchester">platform:comprisesInterfacePart some JavaxSoundSampledSpi</rdfs:comment>
	</owl:Class>
	<owl:Class rdf:about="#JavaxSoundMidiAPI">
		<rdfs:subClassOf rdf:resource="&j2se-1_3;JavaxSoundMidiAPI"/>
		<rdfs:comment xml:lang="en">JavaLibrary implementing the javax.sound.midi package for J2SE 1.4</rdfs:comment>
		<rdfs:comment xml:lang="OWLManchester">platform:comprisesInterfacePart some JavaxSoundMidi</rdfs:comment>
	</owl:Class>
	<owl:Class rdf:about="#JavaxSoundMidiSpiAPI">
		<owl:equivalentClass rdf:resource="&j2se-1_3;JavaxSoundMidiSpiAPI"/>
		<rdfs:subClassOf rdf:resource="&java;JavaAPI"/>
		<rdfs:comment xml:lang="en">JavaLibrary implementing the javax.sound.midi.spi package for J2SE 1.4</rdfs:comment>
		<rdfs:comment xml:lang="OWLManchester">platform:comprisesInterfacePart some JavaxSoundMidiSpi</rdfs:comment>
	</owl:Class>
	<owl:Class rdf:about="#JavaxPrintAPI">
		<rdfs:subClassOf rdf:resource="&java;JavaAPI"/>
		<rdfs:comment xml:lang="en">JavaLibrary implementing the javax.print package for J2SE 1.4</rdfs:comment>
		<rdfs:comment xml:lang="OWLManchester">platform:comprisesInterfacePart some JavaxPrint</rdfs:comment>
	</owl:Class>
	<owl:Class rdf:about="#JavaxPrintAttributeAPI">
		<rdfs:subClassOf rdf:resource="&java;JavaAPI"/>
		<rdfs:comment xml:lang="en">JavaLibrary implementing the javax.print.attribute package for J2SE 1.4</rdfs:comment>
		<rdfs:comment xml:lang="OWLManchester">platform:comprisesInterfacePart some JavaxPrintAttribute</rdfs:comment>
	</owl:Class>
	<owl:Class rdf:about="#JavaxPrintAttributeStandardAPI">
		<rdfs:subClassOf rdf:resource="&java;JavaAPI"/>
		<rdfs:comment xml:lang="en">JavaLibrary implementing the javax.print.attribute.standard package for J2SE 1.4</rdfs:comment>
		<rdfs:comment xml:lang="OWLManchester">platform:comprisesInterfacePart some JavaxPrintAttributeStandard</rdfs:comment>
	</owl:Class>
	<owl:Class rdf:about="#JavaxPrintEventAPI">
		<rdfs:subClassOf rdf:resource="&java;JavaAPI"/>
		<rdfs:comment xml:lang="en">JavaLibrary implementing the javax.print.event package for J2SE 1.4</rdfs:comment>
		<rdfs:comment xml:lang="OWLManchester">platform:comprisesInterfacePart some JavaxPrintEvent</rdfs:comment>
	</owl:Class>
	<owl:Class rdf:about="#JavaxSecurityAuthAPI">
		<rdfs:subClassOf rdf:resource="&java;JavaAPI"/>
		<rdfs:comment xml:lang="en">JavaLibrary implementing the javax.security.auth package for J2SE 1.4</rdfs:comment>
		<rdfs:comment xml:lang="OWLManchester">platform:comprisesInterfacePart some JavaxSecurityAuth</rdfs:comment>
	</owl:Class>
	<owl:Class rdf:about="#JavaxSecurityAuthX500API">
		<rdfs:subClassOf rdf:resource="&j2me-pp-1_1;JavaxSecurityAuthX500API"/>
		<rdfs:comment xml:lang="en">JavaLibrary implementing the javax.security.auth.x500 package for J2SE 1.4</rdfs:comment>
		<rdfs:comment xml:lang="OWLManchester">platform:comprisesInterfacePart some JavaxSecurityAuthX500</rdfs:comment>
	</owl:Class>
	<owl:Class rdf:about="#JavaxSecurityAuthCallbackAPI">
		<rdfs:subClassOf rdf:resource="&java;JavaAPI"/>
		<rdfs:comment xml:lang="en">JavaLibrary implementing the javax.security.auth.callback package for J2SE 1.4</rdfs:comment>
		<rdfs:comment xml:lang="OWLManchester">platform:comprisesInterfacePart some JavaxSecurityAuthCallback</rdfs:comment>
	</owl:Class>
	<owl:Class rdf:about="#JavaxSecurityAuthKerberosAPI">
		<rdfs:subClassOf rdf:resource="&java;JavaAPI"/>
		<rdfs:comment xml:lang="en">JavaLibrary implementing the javax.security.auth.kerberos package for J2SE 1.4</rdfs:comment>
		<rdfs:comment xml:lang="OWLManchester">platform:comprisesInterfacePart some JavaxSecurityAuthKerberos</rdfs:comment>
	</owl:Class>
	<owl:Class rdf:about="#JavaxSecurityAuthLoginAPI">
		<rdfs:subClassOf rdf:resource="&java;JavaAPI"/>
		<rdfs:comment xml:lang="en">JavaLibrary implementing the javax.security.auth.login package for J2SE 1.4</rdfs:comment>
		<rdfs:comment xml:lang="OWLManchester">platform:comprisesInterfacePart some JavaxSecurityAuthLogin</rdfs:comment>
	</owl:Class>
	<owl:Class rdf:about="#JavaxSecurityAuthSpiAPI">
		<rdfs:subClassOf rdf:resource="&java;JavaAPI"/>
		<rdfs:comment xml:lang="en">JavaLibrary implementing the javax.security.auth.spi package for J2SE 1.4</rdfs:comment>
		<rdfs:comment xml:lang="OWLManchester">platform:comprisesInterfacePart some JavaxSecurityAuthSpi</rdfs:comment>
	</owl:Class>
	<owl:Class rdf:about="#JavaxSecurityCertAPI">
		<rdfs:subClassOf rdf:resource="&java;JavaAPI"/>
		<rdfs:comment xml:lang="en">JavaLibrary implementing the javax.security.cert package for J2SE 1.4</rdfs:comment>
		<rdfs:comment xml:lang="OWLManchester">platform:comprisesInterfacePart some JavaxSecurityCert</rdfs:comment>
	</owl:Class>
	<owl:Class rdf:about="#JavaxNamingAPI">
		<rdfs:subClassOf rdf:resource="&j2se-1_3;JavaxNamingAPI"/>
		<rdfs:comment xml:lang="en">JavaLibrary implementing the javax.naming package for J2SE 1.4</rdfs:comment>
		<rdfs:comment xml:lang="OWLManchester">platform:comprisesInterfacePart some JavaxNaming</rdfs:comment>
	</owl:Class>
	<owl:Class rdf:about="#JavaxNamingDirectoryAPI">
		<rdfs:subClassOf rdf:resource="&j2se-1_3;JavaxNamingDirectoryAPI"/>
		<rdfs:comment xml:lang="en">JavaLibrary implementing the javax.naming.directory package for J2SE 1.4</rdfs:comment>
		<rdfs:comment xml:lang="OWLManchester">platform:comprisesInterfacePart some JavaxNamingDirectory</rdfs:comment>
	</owl:Class>
	<owl:Class rdf:about="#JavaxNamingEventAPI">
		<owl:equivalentClass rdf:resource="&j2se-1_3;JavaxNamingEventAPI"/>
		<rdfs:subClassOf rdf:resource="&java;JavaAPI"/>
		<rdfs:comment xml:lang="en">JavaLibrary implementing the javax.naming.event package for J2SE 1.4</rdfs:comment>
		<rdfs:comment xml:lang="OWLManchester">platform:comprisesInterfacePart some JavaxNamingEvent</rdfs:comment>
	</owl:Class>
	<owl:Class rdf:about="#JavaxNamingLdapAPI">
		<rdfs:subClassOf rdf:resource="&j2se-1_3;JavaxNamingLdapAPI"/>
		<rdfs:comment xml:lang="en">JavaLibrary implementing the javax.naming.ldap package for J2SE 1.4</rdfs:comment>
		<rdfs:comment xml:lang="OWLManchester">platform:comprisesInterfacePart some JavaxNamingLdap</rdfs:comment>
	</owl:Class>
	<owl:Class rdf:about="#JavaxNamingSpiAPI">
		<owl:equivalentClass rdf:resource="&j2se-1_3;JavaxNamingSpiAPI"/>
		<rdfs:subClassOf rdf:resource="&java;JavaAPI"/>
		<rdfs:comment xml:lang="en">JavaLibrary implementing the javax.naming.spi package for J2SE 1.4</rdfs:comment>
		<rdfs:comment xml:lang="OWLManchester">platform:comprisesInterfacePart some JavaxNamingSpi</rdfs:comment>
	</owl:Class>
	<owl:Class rdf:about="#JavaxNetAPI">
		<rdfs:subClassOf rdf:resource="&java;JavaAPI"/>
		<rdfs:comment xml:lang="en">JavaLibrary implementing the javax.net package for J2SE 1.4</rdfs:comment>
		<rdfs:comment xml:lang="OWLManchester">platform:comprisesInterfacePart some JavaxNet</rdfs:comment>
	</owl:Class>
	<owl:Class rdf:about="#JavaxNetSslAPI">
		<rdfs:subClassOf rdf:resource="&java;JavaAPI"/>
		<rdfs:comment xml:lang="en">JavaLibrary implementing the javax.net.ssl package for J2SE 1.4</rdfs:comment>
		<rdfs:comment xml:lang="OWLManchester">platform:comprisesInterfacePart some JavaxNetSsl</rdfs:comment>
	</owl:Class>
	<owl:Class rdf:about="#JavaxRmiAPI">
		<owl:equivalentClass rdf:resource="&j2se-1_3;JavaxRmiAPI"/>
		<rdfs:subClassOf rdf:resource="&java;JavaAPI"/>
		<rdfs:comment xml:lang="en">JavaLibrary implementing the javax.rmi package for J2SE 1.4</rdfs:comment>
		<rdfs:comment xml:lang="OWLManchester">platform:comprisesInterfacePart some JavaxRmi</rdfs:comment>
	</owl:Class>
	<owl:Class rdf:about="#JavaxRmiCORBAAPI">
		<owl:equivalentClass rdf:resource="&j2se-1_3;JavaxRmiCORBAAPI"/>
		<rdfs:subClassOf rdf:resource="&java;JavaAPI"/>
		<rdfs:comment xml:lang="en">JavaLibrary implementing the javax.rmi.CORBA package for J2SE 1.4</rdfs:comment>
		<rdfs:comment xml:lang="OWLManchester">platform:comprisesInterfacePart some JavaxRmiCORBA</rdfs:comment>
	</owl:Class>
	<owl:Class rdf:about="#JavaxCryptoAPI">
		<rdfs:subClassOf rdf:resource="&java;JavaAPI"/>
		<rdfs:comment xml:lang="en">JavaLibrary implementing the javax.crypto package for J2SE 1.4</rdfs:comment>
		<rdfs:comment xml:lang="OWLManchester">platform:comprisesInterfacePart some JavaxCrypto</rdfs:comment>
	</owl:Class>
	<owl:Class rdf:about="#JavaxCryptoInterfacesAPI">
		<rdfs:subClassOf rdf:resource="&java;JavaAPI"/>
		<rdfs:comment xml:lang="en">JavaLibrary implementing the javax.crypto.interfaces package for J2SE 1.4</rdfs:comment>
		<rdfs:comment xml:lang="OWLManchester">platform:comprisesInterfacePart some JavaxCryptoInterfaces</rdfs:comment>
	</owl:Class>
	<owl:Class rdf:about="#JavaxCryptoSpecAPI">
		<rdfs:subClassOf rdf:resource="&java;JavaAPI"/>
		<rdfs:comment xml:lang="en">JavaLibrary implementing the javax.crypto.spec package for J2SE 1.4</rdfs:comment>
		<rdfs:comment xml:lang="OWLManchester">platform:comprisesInterfacePart some JavaxCryptoSpec</rdfs:comment>
	</owl:Class>
	<owl:Class rdf:about="#JavaxSqlAPI">
		<rdfs:subClassOf rdf:resource="&java;JavaAPI"/>
		<rdfs:comment xml:lang="en">JavaLibrary implementing the javax.sql package for J2SE 1.4</rdfs:comment>
		<rdfs:comment xml:lang="OWLManchester">platform:comprisesInterfacePart some JavaxSql</rdfs:comment>
	</owl:Class>
	<owl:Class rdf:about="#JavaxTransactionAPI">
		<rdfs:subClassOf rdf:resource="&j2se-1_3;JavaxTransactionAPI"/>
		<rdfs:comment xml:lang="en">JavaLibrary implementing the javax.transaction package for J2SE 1.4</rdfs:comment>
		<rdfs:comment xml:lang="OWLManchester">platform:comprisesInterfacePart some JavaxTransaction</rdfs:comment>
	</owl:Class>
	<owl:Class rdf:about="#JavaxTransactionXaAPI">
		<rdfs:subClassOf rdf:resource="&java;JavaAPI"/>
		<rdfs:comment xml:lang="en">JavaLibrary implementing the javax.transaction.xa package for J2SE 1.4</rdfs:comment>
		<rdfs:comment xml:lang="OWLManchester">platform:comprisesInterfacePart some JavaxTransactionXa</rdfs:comment>
	</owl:Class>
	<owl:Class rdf:about="#JavaxXmlParsersAPI">
		<rdfs:subClassOf rdf:resource="&java;JavaAPI"/>
		<rdfs:comment xml:lang="en">JavaLibrary implementing the javax.xml.parsers package for J2SE 1.4</rdfs:comment>
		<rdfs:comment xml:lang="OWLManchester">platform:comprisesInterfacePart some JavaxXmlParsers</rdfs:comment>
	</owl:Class>
	<owl:Class rdf:about="#JavaxXmlTransformAPI">
		<rdfs:subClassOf rdf:resource="&java;JavaAPI"/>
		<rdfs:comment xml:lang="en">JavaLibrary implementing the javax.xml.transform package for J2SE 1.4</rdfs:comment>
		<rdfs:comment xml:lang="OWLManchester">platform:comprisesInterfacePart some JavaxXmlTransform</rdfs:comment>
	</owl:Class>
	<owl:Class rdf:about="#JavaxXmlTransformDomAPI">
		<rdfs:subClassOf rdf:resource="&java;JavaAPI"/>
		<rdfs:comment xml:lang="en">JavaLibrary implementing the javax.xml.transform.dom package for J2SE 1.4</rdfs:comment>
		<rdfs:comment xml:lang="OWLManchester">platform:comprisesInterfacePart some JavaxXmlTransformDom</rdfs:comment>
	</owl:Class>
	<owl:Class rdf:about="#JavaxXmlTransformSaxAPI">
		<rdfs:subClassOf rdf:resource="&java;JavaAPI"/>
		<rdfs:comment xml:lang="en">JavaLibrary implementing the javax.xml.transform.sax package for J2SE 1.4</rdfs:comment>
		<rdfs:comment xml:lang="OWLManchester">platform:comprisesInterfacePart some JavaxXmlTransformSax</rdfs:comment>
	</owl:Class>
	<owl:Class rdf:about="#JavaxXmlTransformStreamAPI">
		<rdfs:subClassOf rdf:resource="&java;JavaAPI"/>
		<rdfs:comment xml:lang="en">JavaLibrary implementing the javax.xml.transform.stream package for J2SE 1.4</rdfs:comment>
		<rdfs:comment xml:lang="OWLManchester">platform:comprisesInterfacePart some JavaxXmlTransformStream</rdfs:comment>
	</owl:Class>
	<owl:Class rdf:about="#OrgW3cDomAPI">
		<rdfs:subClassOf rdf:resource="&java;JavaAPI"/>
		<rdfs:comment xml:lang="en">JavaLibrary implementing the org.w3c.dom package for J2SE 1.4</rdfs:comment>
		<rdfs:comment xml:lang="OWLManchester">platform:comprisesInterfacePart some OrgW3cDom</rdfs:comment>
	</owl:Class>
	<owl:Class rdf:about="#OrgW3cDomCssAPI">
		<rdfs:subClassOf rdf:resource="&java;JavaAPI"/>
		<rdfs:comment xml:lang="en">JavaLibrary implementing the org.w3c.dom.css package for J2SE 1.4</rdfs:comment>
		<rdfs:comment xml:lang="OWLManchester">platform:comprisesInterfacePart some OrgW3cDomCss</rdfs:comment>
	</owl:Class>
	<owl:Class rdf:about="#OrgW3cDomStylesheetsAPI">
		<rdfs:subClassOf rdf:resource="&java;JavaAPI"/>
		<rdfs:comment xml:lang="en">JavaLibrary implementing the org.w3c.dom.stylesheets package for J2SE 1.4</rdfs:comment>
		<rdfs:comment xml:lang="OWLManchester">platform:comprisesInterfacePart some OrgW3cDomStylesheets</rdfs:comment>
	</owl:Class>
	<owl:Class rdf:about="#OrgW3cDomViewsAPI">
		<rdfs:subClassOf rdf:resource="&java;JavaAPI"/>
		<rdfs:comment xml:lang="en">JavaLibrary implementing the org.w3c.dom.views package for J2SE 1.4</rdfs:comment>
		<rdfs:comment xml:lang="OWLManchester">platform:comprisesInterfacePart some OrgW3cDomViews</rdfs:comment>
	</owl:Class>
	<owl:Class rdf:about="#OrgW3cDomEventsAPI">
		<rdfs:subClassOf rdf:resource="&java;JavaAPI"/>
		<rdfs:comment xml:lang="en">JavaLibrary implementing the org.w3c.dom.events package for J2SE 1.4</rdfs:comment>
		<rdfs:comment xml:lang="OWLManchester">platform:comprisesInterfacePart some OrgW3cDomEvents</rdfs:comment>
	</owl:Class>
	<owl:Class rdf:about="#OrgW3cDomHtmlAPI">
		<rdfs:subClassOf rdf:resource="&java;JavaAPI"/>
		<rdfs:comment xml:lang="en">JavaLibrary implementing the org.w3c.dom.html package for J2SE 1.4</rdfs:comment>
		<rdfs:comment xml:lang="OWLManchester">platform:comprisesInterfacePart some OrgW3cDomHtml</rdfs:comment>
	</owl:Class>
	<owl:Class rdf:about="#OrgW3cDomTraversalAPI">
		<rdfs:subClassOf rdf:resource="&java;JavaAPI"/>
		<rdfs:comment xml:lang="en">JavaLibrary implementing the org.w3c.dom.traversal package for J2SE 1.4</rdfs:comment>
		<rdfs:comment xml:lang="OWLManchester">platform:comprisesInterfacePart some OrgW3cDomTraversal</rdfs:comment>
	</owl:Class>
	<owl:Class rdf:about="#OrgOmgCORBA_2_3API">
		<owl:equivalentClass rdf:resource="&j2se-1_3;OrgOmgCORBA_2_3API"/>
		<rdfs:subClassOf rdf:resource="&java;JavaAPI"/>
		<rdfs:comment xml:lang="en">JavaLibrary implementing the org.omg.CORBA_2_3 package for J2SE 1.4</rdfs:comment>
		<rdfs:comment xml:lang="OWLManchester">platform:comprisesInterfacePart some OrgOmgCORBA_2_3</rdfs:comment>
	</owl:Class>
	<owl:Class rdf:about="#OrgOmgCORBA_2_3PortableAPI">
		<rdfs:subClassOf rdf:resource="&java;JavaAPI"/>
		<rdfs:comment xml:lang="en">JavaLibrary implementing the org.omg.CORBA_2_3.portable package for J2SE 1.4</rdfs:comment>
		<rdfs:comment xml:lang="OWLManchester">platform:comprisesInterfacePart some OrgOmgCORBA_2_3Portable</rdfs:comment>
	</owl:Class>
	<owl:Class rdf:about="#OrgOmgCORBAAPI">
		<rdfs:subClassOf rdf:resource="&java;JavaAPI"/>
		<rdfs:comment xml:lang="en">JavaLibrary implementing the org.omg.CORBA package for J2SE 1.4</rdfs:comment>
		<rdfs:comment xml:lang="OWLManchester">platform:comprisesInterfacePart some OrgOmgCORBA</rdfs:comment>
	</owl:Class>
	<owl:Class rdf:about="#OrgOmgCORBAPortableAPI">
		<rdfs:subClassOf rdf:resource="&java;JavaAPI"/>
		<rdfs:comment xml:lang="en">JavaLibrary implementing the org.omg.CORBA.portable package for J2SE 1.4</rdfs:comment>
		<rdfs:comment xml:lang="OWLManchester">platform:comprisesInterfacePart some OrgOmgCORBAPortable</rdfs:comment>
	</owl:Class>
	<owl:Class rdf:about="#OrgOmgCORBADynAnyPackageAPI">
		<rdfs:subClassOf rdf:resource="&j2se-1_3;OrgOmgCORBADynAnyPackageAPI"/>
		<rdfs:comment xml:lang="en">JavaLibrary implementing the org.omg.CORBA.DynAnyPackage package for J2SE 1.4</rdfs:comment>
		<rdfs:comment xml:lang="OWLManchester">platform:comprisesInterfacePart some OrgOmgCORBADynAnyPackage</rdfs:comment>
	</owl:Class>
	<owl:Class rdf:about="#OrgOmgCORBAORBPackageAPI">
		<rdfs:subClassOf rdf:resource="&j2se-1_3;OrgOmgCORBAORBPackageAPI"/>
		<rdfs:comment xml:lang="en">JavaLibrary implementing the org.omg.CORBA.ORBPackage package for J2SE 1.4</rdfs:comment>
		<rdfs:comment xml:lang="OWLManchester">platform:comprisesInterfacePart some OrgOmgCORBAORBPackage</rdfs:comment>
	</owl:Class>
	<owl:Class rdf:about="#OrgOmgCORBATypeCodePackageAPI">
		<rdfs:subClassOf rdf:resource="&j2se-1_3;OrgOmgCORBATypeCodePackageAPI"/>
		<rdfs:comment xml:lang="en">JavaLibrary implementing the org.omg.CORBA.TypeCodePackage package for J2SE 1.4</rdfs:comment>
		<rdfs:comment xml:lang="OWLManchester">platform:comprisesInterfacePart some OrgOmgCORBATypeCodePackage</rdfs:comment>
	</owl:Class>
	<owl:Class rdf:about="#OrgOmgSendingContextAPI">
		<owl:equivalentClass rdf:resource="&j2se-1_3;OrgOmgSendingContextAPI"/>
		<rdfs:subClassOf rdf:resource="&java;JavaAPI"/>
		<rdfs:comment xml:lang="en">JavaLibrary implementing the org.omg.SendingContext package for J2SE 1.4</rdfs:comment>
		<rdfs:comment xml:lang="OWLManchester">platform:comprisesInterfacePart some OrgOmgSendingContext</rdfs:comment>
	</owl:Class>
	<owl:Class rdf:about="#OrgOmgCosNamingAPI">
		<rdfs:subClassOf rdf:resource="&java;JavaAPI"/>
		<rdfs:comment xml:lang="en">JavaLibrary implementing the org.omg.CosNaming package for J2SE 1.4</rdfs:comment>
		<rdfs:comment xml:lang="OWLManchester">platform:comprisesInterfacePart some OrgOmgCosNaming</rdfs:comment>
	</owl:Class>
	<owl:Class rdf:about="#OrgOmgCosNamingNamingContextExtPackageAPI">
		<rdfs:subClassOf rdf:resource="&java;JavaAPI"/>
		<rdfs:comment xml:lang="en">JavaLibrary implementing the org.omg.CosNaming.NamingContextExtPackage package for J2SE 1.4</rdfs:comment>
		<rdfs:comment xml:lang="OWLManchester">platform:comprisesInterfacePart some OrgOmgCosNamingNamingContextExtPackage</rdfs:comment>
	</owl:Class>
	<owl:Class rdf:about="#OrgOmgCosNamingNamingContextPackageAPI">
		<rdfs:subClassOf rdf:resource="&java;JavaAPI"/>
		<rdfs:comment xml:lang="en">JavaLibrary implementing the org.omg.CosNaming.NamingContextPackage package for J2SE 1.4</rdfs:comment>
		<rdfs:comment xml:lang="OWLManchester">platform:comprisesInterfacePart some OrgOmgCosNamingNamingContextPackage</rdfs:comment>
	</owl:Class>
	<owl:Class rdf:about="#OrgOmgPortableServerAPI">
		<rdfs:subClassOf rdf:resource="&java;JavaAPI"/>
		<rdfs:comment xml:lang="en">JavaLibrary implementing the org.omg.PortableServer package for J2SE 1.4</rdfs:comment>
		<rdfs:comment xml:lang="OWLManchester">platform:comprisesInterfacePart some OrgOmgPortableServer</rdfs:comment>
	</owl:Class>
	<owl:Class rdf:about="#OrgOmgPortableServerCurrentPackageAPI">
		<rdfs:subClassOf rdf:resource="&java;JavaAPI"/>
		<rdfs:comment xml:lang="en">JavaLibrary implementing the org.omg.PortableServer.CurrentPackage package for J2SE 1.4</rdfs:comment>
		<rdfs:comment xml:lang="OWLManchester">platform:comprisesInterfacePart some OrgOmgPortableServerCurrentPackage</rdfs:comment>
	</owl:Class>
	<owl:Class rdf:about="#OrgOmgPortableServerPOAManagerPackageAPI">
		<rdfs:subClassOf rdf:resource="&java;JavaAPI"/>
		<rdfs:comment xml:lang="en">JavaLibrary implementing the org.omg.PortableServer.POAManagerPackage package for J2SE 1.4</rdfs:comment>
		<rdfs:comment xml:lang="OWLManchester">platform:comprisesInterfacePart some OrgOmgPortableServerPOAManagerPackage</rdfs:comment>
	</owl:Class>
	<owl:Class rdf:about="#OrgOmgPortableServerPOAPackageAPI">
		<rdfs:subClassOf rdf:resource="&java;JavaAPI"/>
		<rdfs:comment xml:lang="en">JavaLibrary implementing the org.omg.PortableServer.POAPackage package for J2SE 1.4</rdfs:comment>
		<rdfs:comment xml:lang="OWLManchester">platform:comprisesInterfacePart some OrgOmgPortableServerPOAPackage</rdfs:comment>
	</owl:Class>
	<owl:Class rdf:about="#OrgOmgPortableServerPortableAPI">
		<rdfs:subClassOf rdf:resource="&java;JavaAPI"/>
		<rdfs:comment xml:lang="en">JavaLibrary implementing the org.omg.PortableServer.portable package for J2SE 1.4</rdfs:comment>
		<rdfs:comment xml:lang="OWLManchester">platform:comprisesInterfacePart some OrgOmgPortableServerPortable</rdfs:comment>
	</owl:Class>
	<owl:Class rdf:about="#OrgOmgPortableServerServantLocatorPackageAPI">
		<rdfs:subClassOf rdf:resource="&java;JavaAPI"/>
		<rdfs:comment xml:lang="en">JavaLibrary implementing the org.omg.PortableServer.ServantLocatorPackage package for J2SE 1.4</rdfs:comment>
		<rdfs:comment xml:lang="OWLManchester">platform:comprisesInterfacePart some OrgOmgPortableServerServantLocatorPackage</rdfs:comment>
	</owl:Class>
	<owl:Class rdf:about="#OrgOmgDynamicAPI">
		<rdfs:subClassOf rdf:resource="&java;JavaAPI"/>
		<rdfs:comment xml:lang="en">JavaLibrary implementing the org.omg.Dynamic package for J2SE 1.4</rdfs:comment>
		<rdfs:comment xml:lang="OWLManchester">platform:comprisesInterfacePart some OrgOmgDynamic</rdfs:comment>
	</owl:Class>
	<owl:Class rdf:about="#OrgOmgDynamicAnyAPI">
		<rdfs:subClassOf rdf:resource="&java;JavaAPI"/>
		<rdfs:comment xml:lang="en">JavaLibrary implementing the org.omg.DynamicAny package for J2SE 1.4</rdfs:comment>
		<rdfs:comment xml:lang="OWLManchester">platform:comprisesInterfacePart some OrgOmgDynamicAny</rdfs:comment>
	</owl:Class>
	<owl:Class rdf:about="#OrgOmgDynamicAnyDynAnyFactoryPackageAPI">
		<rdfs:subClassOf rdf:resource="&java;JavaAPI"/>
		<rdfs:comment xml:lang="en">JavaLibrary implementing the org.omg.DynamicAny.DynAnyFactoryPackage package for J2SE 1.4</rdfs:comment>
		<rdfs:comment xml:lang="OWLManchester">platform:comprisesInterfacePart some OrgOmgDynamicAnyDynAnyFactoryPackage</rdfs:comment>
	</owl:Class>
	<owl:Class rdf:about="#OrgOmgDynamicAnyDynAnyPackageAPI">
		<rdfs:subClassOf rdf:resource="&java;JavaAPI"/>
		<rdfs:comment xml:lang="en">JavaLibrary implementing the org.omg.DynamicAny.DynAnyPackage package for J2SE 1.4</rdfs:comment>
		<rdfs:comment xml:lang="OWLManchester">platform:comprisesInterfacePart some OrgOmgDynamicAnyDynAnyPackage</rdfs:comment>
	</owl:Class>
	<owl:Class rdf:about="#OrgOmgIOPAPI">
		<rdfs:subClassOf rdf:resource="&java;JavaAPI"/>
		<rdfs:comment xml:lang="en">JavaLibrary implementing the org.omg.IOP package for J2SE 1.4</rdfs:comment>
		<rdfs:comment xml:lang="OWLManchester">platform:comprisesInterfacePart some OrgOmgIOP</rdfs:comment>
	</owl:Class>
	<owl:Class rdf:about="#OrgOmgIOPCodecFactoryPackageAPI">
		<rdfs:subClassOf rdf:resource="&java;JavaAPI"/>
		<rdfs:comment xml:lang="en">JavaLibrary implementing the org.omg.IOP.CodecFactoryPackage package for J2SE 1.4</rdfs:comment>
		<rdfs:comment xml:lang="OWLManchester">platform:comprisesInterfacePart some OrgOmgIOPCodecFactoryPackage</rdfs:comment>
	</owl:Class>
	<owl:Class rdf:about="#OrgOmgIOPCodecPackageAPI">
		<rdfs:subClassOf rdf:resource="&java;JavaAPI"/>
		<rdfs:comment xml:lang="en">JavaLibrary implementing the org.omg.IOP.CodecPackage package for J2SE 1.4</rdfs:comment>
		<rdfs:comment xml:lang="OWLManchester">platform:comprisesInterfacePart some OrgOmgIOPCodecPackage</rdfs:comment>
	</owl:Class>
	<owl:Class rdf:about="#OrgOmgMessagingAPI">
		<rdfs:subClassOf rdf:resource="&java;JavaAPI"/>
		<rdfs:comment xml:lang="en">JavaLibrary implementing the org.omg.Messaging package for J2SE 1.4</rdfs:comment>
		<rdfs:comment xml:lang="OWLManchester">platform:comprisesInterfacePart some OrgOmgMessaging</rdfs:comment>
	</owl:Class>
	<owl:Class rdf:about="#OrgOmgPortableInterceptorAPI">
		<rdfs:subClassOf rdf:resource="&java;JavaAPI"/>
		<rdfs:comment xml:lang="en">JavaLibrary implementing the org.omg.PortableInterceptor package for J2SE 1.4</rdfs:comment>
		<rdfs:comment xml:lang="OWLManchester">platform:comprisesInterfacePart some OrgOmgPortableInterceptor</rdfs:comment>
	</owl:Class>
	<owl:Class rdf:about="#OrgOmgPortableInterceptorORBInitInfoPackageAPI">
		<rdfs:subClassOf rdf:resource="&java;JavaAPI"/>
		<rdfs:comment xml:lang="en">JavaLibrary implementing the org.omg.PortableInterceptor.ORBInitInfoPackage package for J2SE 1.4</rdfs:comment>
		<rdfs:comment xml:lang="OWLManchester">platform:comprisesInterfacePart some OrgOmgPortableInterceptorORBInitInfoPackage</rdfs:comment>
	</owl:Class>
	<owl:Class rdf:about="#OrgOmgStubJavaRmiAPI">
		<owl:equivalentClass rdf:resource="&j2se-1_3;OrgOmgStubJavaRmiAPI"/>
		<rdfs:subClassOf rdf:resource="&java;JavaAPI"/>
		<rdfs:comment xml:lang="en">JavaLibrary implementing the org.omg.stub.java.rmi package for J2SE 1.4</rdfs:comment>
		<rdfs:comment xml:lang="OWLManchester">platform:comprisesInterfacePart some OrgOmgStubJavaRmi</rdfs:comment>
	</owl:Class>
	<owl:Class rdf:about="#OrgXmlSaxAPI">
		<rdfs:subClassOf rdf:resource="&java;JavaAPI"/>
		<rdfs:comment xml:lang="en">JavaLibrary implementing the org.xml.sax package for J2SE 1.4</rdfs:comment>
		<rdfs:comment xml:lang="OWLManchester">platform:comprisesInterfacePart some OrgXmlSax</rdfs:comment>
	</owl:Class>
	<owl:Class rdf:about="#OrgXmlSaxHelpersAPI">
		<rdfs:subClassOf rdf:resource="&java;JavaAPI"/>
		<rdfs:comment xml:lang="en">JavaLibrary implementing the org.xml.sax.helpers package for J2SE 1.4</rdfs:comment>
		<rdfs:comment xml:lang="OWLManchester">platform:comprisesInterfacePart some OrgXmlSaxHelpers</rdfs:comment>
	</owl:Class>
	<owl:Class rdf:about="#OrgXmlSaxExtAPI">
		<rdfs:subClassOf rdf:resource="&java;JavaAPI"/>
		<rdfs:comment xml:lang="en">JavaLibrary implementing the org.xml.sax.ext package for J2SE 1.4</rdfs:comment>
		<rdfs:comment xml:lang="OWLManchester">platform:comprisesInterfacePart some OrgXmlSaxExt</rdfs:comment>
	</owl:Class>
	<owl:Class rdf:about="#OrgIetfJgssAPI">
		<rdfs:subClassOf rdf:resource="&java;JavaAPI"/>
		<rdfs:comment xml:lang="en">JavaLibrary implementing the org.ietf.jgss package for J2SE 1.4</rdfs:comment>
		<rdfs:comment xml:lang="OWLManchester">platform:comprisesInterfacePart some OrgIetfJgss</rdfs:comment>
	</owl:Class>
	<JavaLang rdf:about="#theJavaLangPart">
	</JavaLang>
	<JavaLangReflect rdf:about="#theJavaLangReflectPart">
	</JavaLangReflect>
	<JavaLangRef rdf:about="#theJavaLangRefPart">
	</JavaLangRef>
	<JavaIo rdf:about="#theJavaIoPart">
	</JavaIo>
	<JavaUtil rdf:about="#theJavaUtilPart">
	</JavaUtil>
	<JavaUtilLogging rdf:about="#theJavaUtilLoggingPart">
	</JavaUtilLogging>
	<JavaUtilJar rdf:about="#theJavaUtilJarPart">
	</JavaUtilJar>
	<JavaUtilZip rdf:about="#theJavaUtilZipPart">
	</JavaUtilZip>
	<JavaUtilPrefs rdf:about="#theJavaUtilPrefsPart">
	</JavaUtilPrefs>
	<JavaUtilRegex rdf:about="#theJavaUtilRegexPart">
	</JavaUtilRegex>
	<JavaNet rdf:about="#theJavaNetPart">
	</JavaNet>
	<JavaSecurity rdf:about="#theJavaSecurityPart">
	</JavaSecurity>
	<JavaSecurityCert rdf:about="#theJavaSecurityCertPart">
	</JavaSecurityCert>
	<JavaSecuritySpec rdf:about="#theJavaSecuritySpecPart">
	</JavaSecuritySpec>
	<JavaSecurityAcl rdf:about="#theJavaSecurityAclPart">
	</JavaSecurityAcl>
	<JavaSecurityInterfaces rdf:about="#theJavaSecurityInterfacesPart">
	</JavaSecurityInterfaces>
	<JavaNio rdf:about="#theJavaNioPart">
	</JavaNio>
	<JavaNioChannels rdf:about="#theJavaNioChannelsPart">
	</JavaNioChannels>
	<JavaNioChannelsSpi rdf:about="#theJavaNioChannelsSpiPart">
	</JavaNioChannelsSpi>
	<JavaNioCharset rdf:about="#theJavaNioCharsetPart">
	</JavaNioCharset>
	<JavaNioCharsetSpi rdf:about="#theJavaNioCharsetSpiPart">
	</JavaNioCharsetSpi>
	<JavaBeans rdf:about="#theJavaBeansPart">
	</JavaBeans>
	<JavaBeansBeancontext rdf:about="#theJavaBeansBeancontextPart">
	</JavaBeansBeancontext>
	<JavaAwt rdf:about="#theJavaAwtPart">
	</JavaAwt>
	<JavaAwtImage rdf:about="#theJavaAwtImagePart">
	</JavaAwtImage>
	<JavaAwtImageRenderable rdf:about="#theJavaAwtImageRenderablePart">
	</JavaAwtImageRenderable>
	<JavaAwtDatatransfer rdf:about="#theJavaAwtDatatransferPart">
	</JavaAwtDatatransfer>
	<JavaAwtDnd rdf:about="#theJavaAwtDndPart">
	</JavaAwtDnd>
	<JavaAwtEvent rdf:about="#theJavaAwtEventPart">
	</JavaAwtEvent>
	<JavaAwtIm rdf:about="#theJavaAwtImPart">
	</JavaAwtIm>
	<JavaAwtImSpi rdf:about="#theJavaAwtImSpiPart">
	</JavaAwtImSpi>
	<JavaAwtFont rdf:about="#theJavaAwtFontPart">
	</JavaAwtFont>
	<JavaAwtGeom rdf:about="#theJavaAwtGeomPart">
	</JavaAwtGeom>
	<JavaAwtColor rdf:about="#theJavaAwtColorPart">
	</JavaAwtColor>
	<JavaAwtPrint rdf:about="#theJavaAwtPrintPart">
	</JavaAwtPrint>
	<JavaText rdf:about="#theJavaTextPart">
	</JavaText>
	<JavaMath rdf:about="#theJavaMathPart">
	</JavaMath>
	<JavaApplet rdf:about="#theJavaAppletPart">
	</JavaApplet>
	<JavaRmi rdf:about="#theJavaRmiPart">
	</JavaRmi>
	<JavaRmiActivation rdf:about="#theJavaRmiActivationPart">
	</JavaRmiActivation>
	<JavaRmiServer rdf:about="#theJavaRmiServerPart">
	</JavaRmiServer>
	<JavaRmiDgc rdf:about="#theJavaRmiDgcPart">
	</JavaRmiDgc>
	<JavaRmiRegistry rdf:about="#theJavaRmiRegistryPart">
	</JavaRmiRegistry>
	<JavaSql rdf:about="#theJavaSqlPart">
	</JavaSql>
	<JavaxImageio rdf:about="#theJavaxImageioPart">
	</JavaxImageio>
	<JavaxImageioSpi rdf:about="#theJavaxImageioSpiPart">
	</JavaxImageioSpi>
	<JavaxImageioMetadata rdf:about="#theJavaxImageioMetadataPart">
	</JavaxImageioMetadata>
	<JavaxImageioStream rdf:about="#theJavaxImageioStreamPart">
	</JavaxImageioStream>
	<JavaxImageioEvent rdf:about="#theJavaxImageioEventPart">
	</JavaxImageioEvent>
	<JavaxImageioPluginsJpeg rdf:about="#theJavaxImageioPluginsJpegPart">
	</JavaxImageioPluginsJpeg>
	<JavaxAccessibility rdf:about="#theJavaxAccessibilityPart">
	</JavaxAccessibility>
	<JavaxSwing rdf:about="#theJavaxSwingPart">
	</JavaxSwing>
	<JavaxSwingPlaf rdf:about="#theJavaxSwingPlafPart">
	</JavaxSwingPlaf>
	<JavaxSwingPlafBasic rdf:about="#theJavaxSwingPlafBasicPart">
	</JavaxSwingPlafBasic>
	<JavaxSwingPlafMetal rdf:about="#theJavaxSwingPlafMetalPart">
	</JavaxSwingPlafMetal>
	<JavaxSwingPlafMulti rdf:about="#theJavaxSwingPlafMultiPart">
	</JavaxSwingPlafMulti>
	<JavaxSwingEvent rdf:about="#theJavaxSwingEventPart">
	</JavaxSwingEvent>
	<JavaxSwingBorder rdf:about="#theJavaxSwingBorderPart">
	</JavaxSwingBorder>
	<JavaxSwingText rdf:about="#theJavaxSwingTextPart">
	</JavaxSwingText>
	<JavaxSwingTextHtml rdf:about="#theJavaxSwingTextHtmlPart">
	</JavaxSwingTextHtml>
	<JavaxSwingTextHtmlParser rdf:about="#theJavaxSwingTextHtmlParserPart">
	</JavaxSwingTextHtmlParser>
	<JavaxSwingTextRtf rdf:about="#theJavaxSwingTextRtfPart">
	</JavaxSwingTextRtf>
	<JavaxSwingTable rdf:about="#theJavaxSwingTablePart">
	</JavaxSwingTable>
	<JavaxSwingUndo rdf:about="#theJavaxSwingUndoPart">
	</JavaxSwingUndo>
	<JavaxSwingTree rdf:about="#theJavaxSwingTreePart">
	</JavaxSwingTree>
	<JavaxSwingFilechooser rdf:about="#theJavaxSwingFilechooserPart">
	</JavaxSwingFilechooser>
	<JavaxSwingColorchooser rdf:about="#theJavaxSwingColorchooserPart">
	</JavaxSwingColorchooser>
	<JavaxSoundSampled rdf:about="#theJavaxSoundSampledPart">
	</JavaxSoundSampled>
	<JavaxSoundSampledSpi rdf:about="#theJavaxSoundSampledSpiPart">
	</JavaxSoundSampledSpi>
	<JavaxSoundMidi rdf:about="#theJavaxSoundMidiPart">
	</JavaxSoundMidi>
	<JavaxSoundMidiSpi rdf:about="#theJavaxSoundMidiSpiPart">
	</JavaxSoundMidiSpi>
	<JavaxPrint rdf:about="#theJavaxPrintPart">
	</JavaxPrint>
	<JavaxPrintAttribute rdf:about="#theJavaxPrintAttributePart">
	</JavaxPrintAttribute>
	<JavaxPrintAttributeStandard rdf:about="#theJavaxPrintAttributeStandardPart">
	</JavaxPrintAttributeStandard>
	<JavaxPrintEvent rdf:about="#theJavaxPrintEventPart">
	</JavaxPrintEvent>
	<JavaxSecurityAuth rdf:about="#theJavaxSecurityAuthPart">
	</JavaxSecurityAuth>
	<JavaxSecurityAuthX500 rdf:about="#theJavaxSecurityAuthX500Part">
	</JavaxSecurityAuthX500>
	<JavaxSecurityAuthCallback rdf:about="#theJavaxSecurityAuthCallbackPart">
	</JavaxSecurityAuthCallback>
	<JavaxSecurityAuthKerberos rdf:about="#theJavaxSecurityAuthKerberosPart">
	</JavaxSecurityAuthKerberos>
	<JavaxSecurityAuthLogin rdf:about="#theJavaxSecurityAuthLoginPart">
	</JavaxSecurityAuthLogin>
	<JavaxSecurityAuthSpi rdf:about="#theJavaxSecurityAuthSpiPart">
	</JavaxSecurityAuthSpi>
	<JavaxSecurityCert rdf:about="#theJavaxSecurityCertPart">
	</JavaxSecurityCert>
	<JavaxNaming rdf:about="#theJavaxNamingPart">
	</JavaxNaming>
	<JavaxNamingDirectory rdf:about="#theJavaxNamingDirectoryPart">
	</JavaxNamingDirectory>
	<JavaxNamingEvent rdf:about="#theJavaxNamingEventPart">
	</JavaxNamingEvent>
	<JavaxNamingLdap rdf:about="#theJavaxNamingLdapPart">
	</JavaxNamingLdap>
	<JavaxNamingSpi rdf:about="#theJavaxNamingSpiPart">
	</JavaxNamingSpi>
	<JavaxNet rdf:about="#theJavaxNetPart">
	</JavaxNet>
	<JavaxNetSsl rdf:about="#theJavaxNetSslPart">
	</JavaxNetSsl>
	<JavaxRmi rdf:about="#theJavaxRmiPart">
	</JavaxRmi>
	<JavaxRmiCORBA rdf:about="#theJavaxRmiCORBAPart">
	</JavaxRmiCORBA>
	<JavaxCrypto rdf:about="#theJavaxCryptoPart">
	</JavaxCrypto>
	<JavaxCryptoInterfaces rdf:about="#theJavaxCryptoInterfacesPart">
	</JavaxCryptoInterfaces>
	<JavaxCryptoSpec rdf:about="#theJavaxCryptoSpecPart">
	</JavaxCryptoSpec>
	<JavaxSql rdf:about="#theJavaxSqlPart">
	</JavaxSql>
	<JavaxTransaction rdf:about="#theJavaxTransactionPart">
	</JavaxTransaction>
	<JavaxTransactionXa rdf:about="#theJavaxTransactionXaPart">
	</JavaxTransactionXa>
	<JavaxXmlParsers rdf:about="#theJavaxXmlParsersPart">
	</JavaxXmlParsers>
	<JavaxXmlTransform rdf:about="#theJavaxXmlTransformPart">
	</JavaxXmlTransform>
	<JavaxXmlTransformDom rdf:about="#theJavaxXmlTransformDomPart">
	</JavaxXmlTransformDom>
	<JavaxXmlTransformSax rdf:about="#theJavaxXmlTransformSaxPart">
	</JavaxXmlTransformSax>
	<JavaxXmlTransformStream rdf:about="#theJavaxXmlTransformStreamPart">
	</JavaxXmlTransformStream>
	<OrgW3cDom rdf:about="#theOrgW3cDomPart">
	</OrgW3cDom>
	<OrgW3cDomCss rdf:about="#theOrgW3cDomCssPart">
	</OrgW3cDomCss>
	<OrgW3cDomStylesheets rdf:about="#theOrgW3cDomStylesheetsPart">
	</OrgW3cDomStylesheets>
	<OrgW3cDomViews rdf:about="#theOrgW3cDomViewsPart">
	</OrgW3cDomViews>
	<OrgW3cDomEvents rdf:about="#theOrgW3cDomEventsPart">
	</OrgW3cDomEvents>
	<OrgW3cDomHtml rdf:about="#theOrgW3cDomHtmlPart">
	</OrgW3cDomHtml>
	<OrgW3cDomTraversal rdf:about="#theOrgW3cDomTraversalPart">
	</OrgW3cDomTraversal>
	<OrgOmgCORBA_2_3 rdf:about="#theOrgOmgCORBA_2_3Part">
	</OrgOmgCORBA_2_3>
	<OrgOmgCORBA_2_3Portable rdf:about="#theOrgOmgCORBA_2_3PortablePart">
	</OrgOmgCORBA_2_3Portable>
	<OrgOmgCORBA rdf:about="#theOrgOmgCORBAPart">
	</OrgOmgCORBA>
	<OrgOmgCORBAPortable rdf:about="#theOrgOmgCORBAPortablePart">
	</OrgOmgCORBAPortable>
	<OrgOmgCORBADynAnyPackage rdf:about="#theOrgOmgCORBADynAnyPackagePart">
	</OrgOmgCORBADynAnyPackage>
	<OrgOmgCORBAORBPackage rdf:about="#theOrgOmgCORBAORBPackagePart">
	</OrgOmgCORBAORBPackage>
	<OrgOmgCORBATypeCodePackage rdf:about="#theOrgOmgCORBATypeCodePackagePart">
	</OrgOmgCORBATypeCodePackage>
	<OrgOmgSendingContext rdf:about="#theOrgOmgSendingContextPart">
	</OrgOmgSendingContext>
	<OrgOmgCosNaming rdf:about="#theOrgOmgCosNamingPart">
	</OrgOmgCosNaming>
	<OrgOmgCosNamingNamingContextExtPackage rdf:about="#theOrgOmgCosNamingNamingContextExtPackagePart">
	</OrgOmgCosNamingNamingContextExtPackage>
	<OrgOmgCosNamingNamingContextPackage rdf:about="#theOrgOmgCosNamingNamingContextPackagePart">
	</OrgOmgCosNamingNamingContextPackage>
	<OrgOmgPortableServer rdf:about="#theOrgOmgPortableServerPart">
	</OrgOmgPortableServer>
	<OrgOmgPortableServerCurrentPackage rdf:about="#theOrgOmgPortableServerCurrentPackagePart">
	</OrgOmgPortableServerCurrentPackage>
	<OrgOmgPortableServerPOAManagerPackage rdf:about="#theOrgOmgPortableServerPOAManagerPackagePart">
	</OrgOmgPortableServerPOAManagerPackage>
	<OrgOmgPortableServerPOAPackage rdf:about="#theOrgOmgPortableServerPOAPackagePart">
	</OrgOmgPortableServerPOAPackage>
	<OrgOmgPortableServerPortable rdf:about="#theOrgOmgPortableServerPortablePart">
	</OrgOmgPortableServerPortable>
	<OrgOmgPortableServerServantLocatorPackage rdf:about="#theOrgOmgPortableServerServantLocatorPackagePart">
	</OrgOmgPortableServerServantLocatorPackage>
	<OrgOmgDynamic rdf:about="#theOrgOmgDynamicPart">
	</OrgOmgDynamic>
	<OrgOmgDynamicAny rdf:about="#theOrgOmgDynamicAnyPart">
	</OrgOmgDynamicAny>
	<OrgOmgDynamicAnyDynAnyFactoryPackage rdf:about="#theOrgOmgDynamicAnyDynAnyFactoryPackagePart">
	</OrgOmgDynamicAnyDynAnyFactoryPackage>
	<OrgOmgDynamicAnyDynAnyPackage rdf:about="#theOrgOmgDynamicAnyDynAnyPackagePart">
	</OrgOmgDynamicAnyDynAnyPackage>
	<OrgOmgIOP rdf:about="#theOrgOmgIOPPart">
	</OrgOmgIOP>
	<OrgOmgIOPCodecFactoryPackage rdf:about="#theOrgOmgIOPCodecFactoryPackagePart">
	</OrgOmgIOPCodecFactoryPackage>
	<OrgOmgIOPCodecPackage rdf:about="#theOrgOmgIOPCodecPackagePart">
	</OrgOmgIOPCodecPackage>
	<OrgOmgMessaging rdf:about="#theOrgOmgMessagingPart">
	</OrgOmgMessaging>
	<OrgOmgPortableInterceptor rdf:about="#theOrgOmgPortableInterceptorPart">
	</OrgOmgPortableInterceptor>
	<OrgOmgPortableInterceptorORBInitInfoPackage rdf:about="#theOrgOmgPortableInterceptorORBInitInfoPackagePart">
	</OrgOmgPortableInterceptorORBInitInfoPackage>
	<OrgOmgStubJavaRmi rdf:about="#theOrgOmgStubJavaRmiPart">
	</OrgOmgStubJavaRmi>
	<OrgXmlSax rdf:about="#theOrgXmlSaxPart">
	</OrgXmlSax>
	<OrgXmlSaxHelpers rdf:about="#theOrgXmlSaxHelpersPart">
	</OrgXmlSaxHelpers>
	<OrgXmlSaxExt rdf:about="#theOrgXmlSaxExtPart">
	</OrgXmlSaxExt>
	<OrgIetfJgss rdf:about="#theOrgIetfJgssPart">
	</OrgIetfJgss>
	<owl:Class rdf:about="#JavaLangClassLibrary">
		<rdfs:subClassOf rdf:resource="&j2me-pp-1_1;JavaLangClassLibrary"/>
		<rdfs:subClassOf rdf:resource="&j2se-1_3;JavaLangClassLibrary"/>
		<rdfs:comment xml:lang="en">JavaLibrary implementing the java.lang package for J2SE 1.4</rdfs:comment>
		<rdfs:comment xml:lang="OWLManchester">platform:implementsInterface some JavaLangAPI</rdfs:comment>
	</owl:Class>
	<owl:Class rdf:about="#JavaLangReflectClassLibrary">
		<owl:equivalentClass rdf:resource="&j2me-pp-1_1;JavaLangReflectClassLibrary"/>
		<rdfs:subClassOf rdf:resource="&j2se-1_3;JavaLangReflectClassLibrary"/>
		<rdfs:comment xml:lang="en">JavaLibrary implementing the java.lang.reflect package for J2SE 1.4</rdfs:comment>
		<rdfs:comment xml:lang="OWLManchester">platform:implementsInterface some JavaLangReflectAPI</rdfs:comment>
	</owl:Class>
	<owl:Class rdf:about="#JavaLangRefClassLibrary">
		<owl:equivalentClass rdf:resource="&j2me-pp-1_1;JavaLangRefClassLibrary"/>
		<owl:equivalentClass rdf:resource="&j2se-1_3;JavaLangRefClassLibrary"/>
		<rdfs:subClassOf rdf:resource="&java;JavaClassLibrary"/>
		<rdfs:comment xml:lang="en">JavaLibrary implementing the java.lang.ref package for J2SE 1.4</rdfs:comment>
		<rdfs:comment xml:lang="OWLManchester">platform:implementsInterface some JavaLangRefAPI</rdfs:comment>
	</owl:Class>
	<owl:Class rdf:about="#JavaIoClassLibrary">
		<rdfs:subClassOf rdf:resource="&j2me-pp-1_1;JavaIoClassLibrary"/>
		<rdfs:subClassOf rdf:resource="&j2se-1_3;JavaIoClassLibrary"/>
		<rdfs:comment xml:lang="en">JavaLibrary implementing the java.io package for J2SE 1.4</rdfs:comment>
		<rdfs:comment xml:lang="OWLManchester">platform:implementsInterface some JavaIoAPI</rdfs:comment>
	</owl:Class>
	<owl:Class rdf:about="#JavaUtilClassLibrary">
		<rdfs:subClassOf rdf:resource="&j2me-pp-1_1;JavaUtilClassLibrary"/>
		<rdfs:subClassOf rdf:resource="&j2se-1_3;JavaUtilClassLibrary"/>
		<rdfs:comment xml:lang="en">JavaLibrary implementing the java.util package for J2SE 1.4</rdfs:comment>
		<rdfs:comment xml:lang="OWLManchester">platform:implementsInterface some JavaUtilAPI</rdfs:comment>
	</owl:Class>
	<owl:Class rdf:about="#JavaUtilLoggingClassLibrary">
		<rdfs:subClassOf rdf:resource="&java;JavaClassLibrary"/>
		<rdfs:comment xml:lang="en">JavaLibrary implementing the java.util.logging package for J2SE 1.4</rdfs:comment>
		<rdfs:comment xml:lang="OWLManchester">platform:implementsInterface some JavaUtilLoggingAPI</rdfs:comment>
	</owl:Class>
	<owl:Class rdf:about="#JavaUtilJarClassLibrary">
		<owl:equivalentClass rdf:resource="&j2me-pp-1_1;JavaUtilJarClassLibrary"/>
		<rdfs:subClassOf rdf:resource="&j2se-1_3;JavaUtilJarClassLibrary"/>
		<rdfs:comment xml:lang="en">JavaLibrary implementing the java.util.jar package for J2SE 1.4</rdfs:comment>
		<rdfs:comment xml:lang="OWLManchester">platform:implementsInterface some JavaUtilJarAPI</rdfs:comment>
	</owl:Class>
	<owl:Class rdf:about="#JavaUtilZipClassLibrary">
		<owl:equivalentClass rdf:resource="&j2me-pp-1_1;JavaUtilZipClassLibrary"/>
		<rdfs:subClassOf rdf:resource="&j2se-1_3;JavaUtilZipClassLibrary"/>
		<rdfs:comment xml:lang="en">JavaLibrary implementing the java.util.zip package for J2SE 1.4</rdfs:comment>
		<rdfs:comment xml:lang="OWLManchester">platform:implementsInterface some JavaUtilZipAPI</rdfs:comment>
	</owl:Class>
	<owl:Class rdf:about="#JavaUtilPrefsClassLibrary">
		<rdfs:subClassOf rdf:resource="&java;JavaClassLibrary"/>
		<rdfs:comment xml:lang="en">JavaLibrary implementing the java.util.prefs package for J2SE 1.4</rdfs:comment>
		<rdfs:comment xml:lang="OWLManchester">platform:implementsInterface some JavaUtilPrefsAPI</rdfs:comment>
	</owl:Class>
	<owl:Class rdf:about="#JavaUtilRegexClassLibrary">
		<rdfs:subClassOf rdf:resource="&java;JavaClassLibrary"/>
		<rdfs:comment xml:lang="en">JavaLibrary implementing the java.util.regex package for J2SE 1.4</rdfs:comment>
		<rdfs:comment xml:lang="OWLManchester">platform:implementsInterface some JavaUtilRegexAPI</rdfs:comment>
	</owl:Class>
	<owl:Class rdf:about="#JavaNetClassLibrary">
		<rdfs:subClassOf rdf:resource="&j2me-pp-1_1;JavaNetClassLibrary"/>
		<rdfs:subClassOf rdf:resource="&j2se-1_3;JavaNetClassLibrary"/>
		<rdfs:comment xml:lang="en">JavaLibrary implementing the java.net package for J2SE 1.4</rdfs:comment>
		<rdfs:comment xml:lang="OWLManchester">platform:implementsInterface some JavaNetAPI</rdfs:comment>
	</owl:Class>
	<owl:Class rdf:about="#JavaSecurityClassLibrary">
		<rdfs:subClassOf rdf:resource="&j2me-pp-1_1;JavaSecurityClassLibrary"/>
		<rdfs:subClassOf rdf:resource="&j2se-1_3;JavaSecurityClassLibrary"/>
		<rdfs:comment xml:lang="en">JavaLibrary implementing the java.security package for J2SE 1.4</rdfs:comment>
		<rdfs:comment xml:lang="OWLManchester">platform:implementsInterface some JavaSecurityAPI</rdfs:comment>
	</owl:Class>
	<owl:Class rdf:about="#JavaSecurityCertClassLibrary">
		<rdfs:subClassOf rdf:resource="&j2me-pp-1_1;JavaSecurityCertClassLibrary"/>
		<rdfs:subClassOf rdf:resource="&j2se-1_3;JavaSecurityCertClassLibrary"/>
		<rdfs:comment xml:lang="en">JavaLibrary implementing the java.security.cert package for J2SE 1.4</rdfs:comment>
		<rdfs:comment xml:lang="OWLManchester">platform:implementsInterface some JavaSecurityCertAPI</rdfs:comment>
	</owl:Class>
	<owl:Class rdf:about="#JavaSecuritySpecClassLibrary">
		<rdfs:subClassOf rdf:resource="&j2me-pp-1_1;JavaSecuritySpecClassLibrary"/>
		<rdfs:subClassOf rdf:resource="&j2se-1_3;JavaSecuritySpecClassLibrary"/>
		<rdfs:comment xml:lang="en">JavaLibrary implementing the java.security.spec package for J2SE 1.4</rdfs:comment>
		<rdfs:comment xml:lang="OWLManchester">platform:implementsInterface some JavaSecuritySpecAPI</rdfs:comment>
	</owl:Class>
	<owl:Class rdf:about="#JavaSecurityAclClassLibrary">
		<owl:equivalentClass rdf:resource="&j2me-pp-1_1;JavaSecurityAclClassLibrary"/>
		<rdfs:subClassOf rdf:resource="&j2se-1_3;JavaSecurityAclClassLibrary"/>
		<rdfs:comment xml:lang="en">JavaLibrary implementing the java.security.acl package for J2SE 1.4</rdfs:comment>
		<rdfs:comment xml:lang="OWLManchester">platform:implementsInterface some JavaSecurityAclAPI</rdfs:comment>
	</owl:Class>
	<owl:Class rdf:about="#JavaSecurityInterfacesClassLibrary">
		<rdfs:subClassOf rdf:resource="&j2me-pp-1_1;JavaSecurityInterfacesClassLibrary"/>
		<rdfs:subClassOf rdf:resource="&j2se-1_3;JavaSecurityInterfacesClassLibrary"/>
		<rdfs:comment xml:lang="en">JavaLibrary implementing the java.security.interfaces package for J2SE 1.4</rdfs:comment>
		<rdfs:comment xml:lang="OWLManchester">platform:implementsInterface some JavaSecurityInterfacesAPI</rdfs:comment>
	</owl:Class>
	<owl:Class rdf:about="#JavaNioClassLibrary">
		<rdfs:subClassOf rdf:resource="&java;JavaClassLibrary"/>
		<rdfs:comment xml:lang="en">JavaLibrary implementing the java.nio package for J2SE 1.4</rdfs:comment>
		<rdfs:comment xml:lang="OWLManchester">platform:implementsInterface some JavaNioAPI</rdfs:comment>
	</owl:Class>
	<owl:Class rdf:about="#JavaNioChannelsClassLibrary">
		<rdfs:subClassOf rdf:resource="&java;JavaClassLibrary"/>
		<rdfs:comment xml:lang="en">JavaLibrary implementing the java.nio.channels package for J2SE 1.4</rdfs:comment>
		<rdfs:comment xml:lang="OWLManchester">platform:implementsInterface some JavaNioChannelsAPI</rdfs:comment>
	</owl:Class>
	<owl:Class rdf:about="#JavaNioChannelsSpiClassLibrary">
		<rdfs:subClassOf rdf:resource="&java;JavaClassLibrary"/>
		<rdfs:comment xml:lang="en">JavaLibrary implementing the java.nio.channels.spi package for J2SE 1.4</rdfs:comment>
		<rdfs:comment xml:lang="OWLManchester">platform:implementsInterface some JavaNioChannelsSpiAPI</rdfs:comment>
	</owl:Class>
	<owl:Class rdf:about="#JavaNioCharsetClassLibrary">
		<rdfs:subClassOf rdf:resource="&java;JavaClassLibrary"/>
		<rdfs:comment xml:lang="en">JavaLibrary implementing the java.nio.charset package for J2SE 1.4</rdfs:comment>
		<rdfs:comment xml:lang="OWLManchester">platform:implementsInterface some JavaNioCharsetAPI</rdfs:comment>
	</owl:Class>
	<owl:Class rdf:about="#JavaNioCharsetSpiClassLibrary">
		<rdfs:subClassOf rdf:resource="&java;JavaClassLibrary"/>
		<rdfs:comment xml:lang="en">JavaLibrary implementing the java.nio.charset.spi package for J2SE 1.4</rdfs:comment>
		<rdfs:comment xml:lang="OWLManchester">platform:implementsInterface some JavaNioCharsetSpiAPI</rdfs:comment>
	</owl:Class>
	<owl:Class rdf:about="#JavaBeansClassLibrary">
		<rdfs:subClassOf rdf:resource="&j2me-pp-1_1;JavaBeansClassLibrary"/>
		<rdfs:subClassOf rdf:resource="&j2se-1_3;JavaBeansClassLibrary"/>
		<rdfs:comment xml:lang="en">JavaLibrary implementing the java.beans package for J2SE 1.4</rdfs:comment>
		<rdfs:comment xml:lang="OWLManchester">platform:implementsInterface some JavaBeansAPI</rdfs:comment>
	</owl:Class>
	<owl:Class rdf:about="#JavaBeansBeancontextClassLibrary">
		<owl:equivalentClass rdf:resource="&j2se-1_3;JavaBeansBeancontextClassLibrary"/>
		<rdfs:subClassOf rdf:resource="&java;JavaClassLibrary"/>
		<rdfs:comment xml:lang="en">JavaLibrary implementing the java.beans.beancontext package for J2SE 1.4</rdfs:comment>
		<rdfs:comment xml:lang="OWLManchester">platform:implementsInterface some JavaBeansBeancontextAPI</rdfs:comment>
	</owl:Class>
	<owl:Class rdf:about="#JavaAwtClassLibrary">
		<rdfs:subClassOf rdf:resource="&j2me-pp-1_1;JavaAwtClassLibrary"/>
		<rdfs:subClassOf rdf:resource="&j2se-1_3;JavaAwtClassLibrary"/>
		<rdfs:comment xml:lang="en">JavaLibrary implementing the java.awt package for J2SE 1.4</rdfs:comment>
		<rdfs:comment xml:lang="OWLManchester">platform:implementsInterface some JavaAwtAPI</rdfs:comment>
	</owl:Class>
	<owl:Class rdf:about="#JavaAwtImageClassLibrary">
		<rdfs:subClassOf rdf:resource="&j2me-pp-1_1;JavaAwtImageClassLibrary"/>
		<rdfs:subClassOf rdf:resource="&j2se-1_3;JavaAwtImageClassLibrary"/>
		<rdfs:comment xml:lang="en">JavaLibrary implementing the java.awt.image package for J2SE 1.4</rdfs:comment>
		<rdfs:comment xml:lang="OWLManchester">platform:implementsInterface some JavaAwtImageAPI</rdfs:comment>
	</owl:Class>
	<owl:Class rdf:about="#JavaAwtImageRenderableClassLibrary">
		<owl:equivalentClass rdf:resource="&j2se-1_3;JavaAwtImageRenderableClassLibrary"/>
		<rdfs:subClassOf rdf:resource="&java;JavaClassLibrary"/>
		<rdfs:comment xml:lang="en">JavaLibrary implementing the java.awt.image.renderable package for J2SE 1.4</rdfs:comment>
		<rdfs:comment xml:lang="OWLManchester">platform:implementsInterface some JavaAwtImageRenderableAPI</rdfs:comment>
	</owl:Class>
	<owl:Class rdf:about="#JavaAwtDatatransferClassLibrary">
		<rdfs:subClassOf rdf:resource="&j2me-pp-1_1;JavaAwtDatatransferClassLibrary"/>
		<rdfs:subClassOf rdf:resource="&j2se-1_3;JavaAwtDatatransferClassLibrary"/>
		<rdfs:comment xml:lang="en">JavaLibrary implementing the java.awt.datatransfer package for J2SE 1.4</rdfs:comment>
		<rdfs:comment xml:lang="OWLManchester">platform:implementsInterface some JavaAwtDatatransferAPI</rdfs:comment>
	</owl:Class>
	<owl:Class rdf:about="#JavaAwtDndClassLibrary">
		<rdfs:subClassOf rdf:resource="&j2se-1_3;JavaAwtDndClassLibrary"/>
		<rdfs:comment xml:lang="en">JavaLibrary implementing the java.awt.dnd package for J2SE 1.4</rdfs:comment>
		<rdfs:comment xml:lang="OWLManchester">platform:implementsInterface some JavaAwtDndAPI</rdfs:comment>
	</owl:Class>
	<owl:Class rdf:about="#JavaAwtEventClassLibrary">
		<rdfs:subClassOf rdf:resource="&j2me-pp-1_1;JavaAwtEventClassLibrary"/>
		<rdfs:subClassOf rdf:resource="&j2se-1_3;JavaAwtEventClassLibrary"/>
		<rdfs:comment xml:lang="en">JavaLibrary implementing the java.awt.event package for J2SE 1.4</rdfs:comment>
		<rdfs:comment xml:lang="OWLManchester">platform:implementsInterface some JavaAwtEventAPI</rdfs:comment>
	</owl:Class>
	<owl:Class rdf:about="#JavaAwtImClassLibrary">
		<owl:equivalentClass rdf:resource="&j2se-1_3;JavaAwtImClassLibrary"/>
		<rdfs:subClassOf rdf:resource="&j2me-pp-1_1;JavaAwtImClassLibrary"/>
		<rdfs:comment xml:lang="en">JavaLibrary implementing the java.awt.im package for J2SE 1.4</rdfs:comment>
		<rdfs:comment xml:lang="OWLManchester">platform:implementsInterface some JavaAwtImAPI</rdfs:comment>
	</owl:Class>
	<owl:Class rdf:about="#JavaAwtImSpiClassLibrary">
		<rdfs:subClassOf rdf:resource="&j2se-1_3;JavaAwtImSpiClassLibrary"/>
		<rdfs:comment xml:lang="en">JavaLibrary implementing the java.awt.im.spi package for J2SE 1.4</rdfs:comment>
		<rdfs:comment xml:lang="OWLManchester">platform:implementsInterface some JavaAwtImSpiAPI</rdfs:comment>
	</owl:Class>
	<owl:Class rdf:about="#JavaAwtFontClassLibrary">
		<rdfs:subClassOf rdf:resource="&j2me-pp-1_1;JavaAwtFontClassLibrary"/>
		<rdfs:subClassOf rdf:resource="&j2se-1_3;JavaAwtFontClassLibrary"/>
		<rdfs:comment xml:lang="en">JavaLibrary implementing the java.awt.font package for J2SE 1.4</rdfs:comment>
		<rdfs:comment xml:lang="OWLManchester">platform:implementsInterface some JavaAwtFontAPI</rdfs:comment>
	</owl:Class>
	<owl:Class rdf:about="#JavaAwtGeomClassLibrary">
		<rdfs:subClassOf rdf:resource="&j2se-1_3;JavaAwtGeomClassLibrary"/>
		<rdfs:comment xml:lang="en">JavaLibrary implementing the java.awt.geom package for J2SE 1.4</rdfs:comment>
		<rdfs:comment xml:lang="OWLManchester">platform:implementsInterface some JavaAwtGeomAPI</rdfs:comment>
	</owl:Class>
	<owl:Class rdf:about="#JavaAwtColorClassLibrary">
		<rdfs:subClassOf rdf:resource="&j2me-pp-1_1;JavaAwtColorClassLibrary"/>
		<rdfs:subClassOf rdf:resource="&j2se-1_3;JavaAwtColorClassLibrary"/>
		<rdfs:comment xml:lang="en">JavaLibrary implementing the java.awt.color package for J2SE 1.4</rdfs:comment>
		<rdfs:comment xml:lang="OWLManchester">platform:implementsInterface some JavaAwtColorAPI</rdfs:comment>
	</owl:Class>
	<owl:Class rdf:about="#JavaAwtPrintClassLibrary">
		<rdfs:subClassOf rdf:resource="&j2se-1_3;JavaAwtPrintClassLibrary"/>
		<rdfs:comment xml:lang="en">JavaLibrary implementing the java.awt.print package for J2SE 1.4</rdfs:comment>
		<rdfs:comment xml:lang="OWLManchester">platform:implementsInterface some JavaAwtPrintAPI</rdfs:comment>
	</owl:Class>
	<owl:Class rdf:about="#JavaTextClassLibrary">
		<rdfs:subClassOf rdf:resource="&j2se-1_3;JavaTextClassLibrary"/>
		<rdfs:comment xml:lang="en">JavaLibrary implementing the java.text package for J2SE 1.4</rdfs:comment>
		<rdfs:comment xml:lang="OWLManchester">platform:implementsInterface some JavaTextAPI</rdfs:comment>
	</owl:Class>
	<owl:Class rdf:about="#JavaMathClassLibrary">
		<rdfs:subClassOf rdf:resource="&j2me-pp-1_1;JavaMathClassLibrary"/>
		<rdfs:subClassOf rdf:resource="&j2se-1_3;JavaMathClassLibrary"/>
		<rdfs:comment xml:lang="en">JavaLibrary implementing the java.math package for J2SE 1.4</rdfs:comment>
		<rdfs:comment xml:lang="OWLManchester">platform:implementsInterface some JavaMathAPI</rdfs:comment>
	</owl:Class>
	<owl:Class rdf:about="#JavaAppletClassLibrary">
		<rdfs:subClassOf rdf:resource="&j2me-pp-1_1;JavaAppletClassLibrary"/>
		<rdfs:subClassOf rdf:resource="&j2se-1_3;JavaAppletClassLibrary"/>
		<rdfs:comment xml:lang="en">JavaLibrary implementing the java.applet package for J2SE 1.4</rdfs:comment>
		<rdfs:comment xml:lang="OWLManchester">platform:implementsInterface some JavaAppletAPI</rdfs:comment>
	</owl:Class>
	<owl:Class rdf:about="#JavaRmiClassLibrary">
		<rdfs:subClassOf rdf:resource="&j2me-pp-1_1;JavaRmiClassLibrary"/>
		<rdfs:subClassOf rdf:resource="&j2se-1_3;JavaRmiClassLibrary"/>
		<rdfs:comment xml:lang="en">JavaLibrary implementing the java.rmi package for J2SE 1.4</rdfs:comment>
		<rdfs:comment xml:lang="OWLManchester">platform:implementsInterface some JavaRmiAPI</rdfs:comment>
	</owl:Class>
	<owl:Class rdf:about="#JavaRmiActivationClassLibrary">
		<rdfs:subClassOf rdf:resource="&j2se-1_3;JavaRmiActivationClassLibrary"/>
		<rdfs:comment xml:lang="en">JavaLibrary implementing the java.rmi.activation package for J2SE 1.4</rdfs:comment>
		<rdfs:comment xml:lang="OWLManchester">platform:implementsInterface some JavaRmiActivationAPI</rdfs:comment>
	</owl:Class>
	<owl:Class rdf:about="#JavaRmiServerClassLibrary">
		<rdfs:subClassOf rdf:resource="&j2se-1_3;JavaRmiServerClassLibrary"/>
		<rdfs:comment xml:lang="en">JavaLibrary implementing the java.rmi.server package for J2SE 1.4</rdfs:comment>
		<rdfs:comment xml:lang="OWLManchester">platform:implementsInterface some JavaRmiServerAPI</rdfs:comment>
	</owl:Class>
	<owl:Class rdf:about="#JavaRmiDgcClassLibrary">
		<owl:equivalentClass rdf:resource="&j2se-1_3;JavaRmiDgcClassLibrary"/>
		<rdfs:subClassOf rdf:resource="&java;JavaClassLibrary"/>
		<rdfs:comment xml:lang="en">JavaLibrary implementing the java.rmi.dgc package for J2SE 1.4</rdfs:comment>
		<rdfs:comment xml:lang="OWLManchester">platform:implementsInterface some JavaRmiDgcAPI</rdfs:comment>
	</owl:Class>
	<owl:Class rdf:about="#JavaRmiRegistryClassLibrary">
		<owl:equivalentClass rdf:resource="&j2se-1_3;JavaRmiRegistryClassLibrary"/>
		<rdfs:subClassOf rdf:resource="&j2me-pp-1_1;JavaRmiRegistryClassLibrary"/>
		<rdfs:comment xml:lang="en">JavaLibrary implementing the java.rmi.registry package for J2SE 1.4</rdfs:comment>
		<rdfs:comment xml:lang="OWLManchester">platform:implementsInterface some JavaRmiRegistryAPI</rdfs:comment>
	</owl:Class>
	<owl:Class rdf:about="#JavaSqlClassLibrary">
		<rdfs:subClassOf rdf:resource="&j2se-1_3;JavaSqlClassLibrary"/>
		<rdfs:comment xml:lang="en">JavaLibrary implementing the java.sql package for J2SE 1.4</rdfs:comment>
		<rdfs:comment xml:lang="OWLManchester">platform:implementsInterface some JavaSqlAPI</rdfs:comment>
	</owl:Class>
	<owl:Class rdf:about="#JavaxImageioClassLibrary">
		<rdfs:subClassOf rdf:resource="&java;JavaClassLibrary"/>
		<rdfs:comment xml:lang="en">JavaLibrary implementing the javax.imageio package for J2SE 1.4</rdfs:comment>
		<rdfs:comment xml:lang="OWLManchester">platform:implementsInterface some JavaxImageioAPI</rdfs:comment>
	</owl:Class>
	<owl:Class rdf:about="#JavaxImageioSpiClassLibrary">
		<rdfs:subClassOf rdf:resource="&java;JavaClassLibrary"/>
		<rdfs:comment xml:lang="en">JavaLibrary implementing the javax.imageio.spi package for J2SE 1.4</rdfs:comment>
		<rdfs:comment xml:lang="OWLManchester">platform:implementsInterface some JavaxImageioSpiAPI</rdfs:comment>
	</owl:Class>
	<owl:Class rdf:about="#JavaxImageioMetadataClassLibrary">
		<rdfs:subClassOf rdf:resource="&java;JavaClassLibrary"/>
		<rdfs:comment xml:lang="en">JavaLibrary implementing the javax.imageio.metadata package for J2SE 1.4</rdfs:comment>
		<rdfs:comment xml:lang="OWLManchester">platform:implementsInterface some JavaxImageioMetadataAPI</rdfs:comment>
	</owl:Class>
	<owl:Class rdf:about="#JavaxImageioStreamClassLibrary">
		<rdfs:subClassOf rdf:resource="&java;JavaClassLibrary"/>
		<rdfs:comment xml:lang="en">JavaLibrary implementing the javax.imageio.stream package for J2SE 1.4</rdfs:comment>
		<rdfs:comment xml:lang="OWLManchester">platform:implementsInterface some JavaxImageioStreamAPI</rdfs:comment>
	</owl:Class>
	<owl:Class rdf:about="#JavaxImageioEventClassLibrary">
		<rdfs:subClassOf rdf:resource="&java;JavaClassLibrary"/>
		<rdfs:comment xml:lang="en">JavaLibrary implementing the javax.imageio.event package for J2SE 1.4</rdfs:comment>
		<rdfs:comment xml:lang="OWLManchester">platform:implementsInterface some JavaxImageioEventAPI</rdfs:comment>
	</owl:Class>
	<owl:Class rdf:about="#JavaxImageioPluginsJpegClassLibrary">
		<rdfs:subClassOf rdf:resource="&java;JavaClassLibrary"/>
		<rdfs:comment xml:lang="en">JavaLibrary implementing the javax.imageio.plugins.jpeg package for J2SE 1.4</rdfs:comment>
		<rdfs:comment xml:lang="OWLManchester">platform:implementsInterface some JavaxImageioPluginsJpegAPI</rdfs:comment>
	</owl:Class>
	<owl:Class rdf:about="#JavaxAccessibilityClassLibrary">
		<rdfs:subClassOf rdf:resource="&j2se-1_3;JavaxAccessibilityClassLibrary"/>
		<rdfs:comment xml:lang="en">JavaLibrary implementing the javax.accessibility package for J2SE 1.4</rdfs:comment>
		<rdfs:comment xml:lang="OWLManchester">platform:implementsInterface some JavaxAccessibilityAPI</rdfs:comment>
	</owl:Class>
	<owl:Class rdf:about="#JavaxSwingClassLibrary">
		<rdfs:subClassOf rdf:resource="&java;JavaClassLibrary"/>
		<rdfs:comment xml:lang="en">JavaLibrary implementing the javax.swing package for J2SE 1.4</rdfs:comment>
		<rdfs:comment xml:lang="OWLManchester">platform:implementsInterface some JavaxSwingAPI</rdfs:comment>
	</owl:Class>
	<owl:Class rdf:about="#JavaxSwingPlafClassLibrary">
		<rdfs:subClassOf rdf:resource="&j2se-1_3;JavaxSwingPlafClassLibrary"/>
		<rdfs:comment xml:lang="en">JavaLibrary implementing the javax.swing.plaf package for J2SE 1.4</rdfs:comment>
		<rdfs:comment xml:lang="OWLManchester">platform:implementsInterface some JavaxSwingPlafAPI</rdfs:comment>
	</owl:Class>
	<owl:Class rdf:about="#JavaxSwingPlafBasicClassLibrary">
		<rdfs:subClassOf rdf:resource="&j2se-1_3;JavaxSwingPlafBasicClassLibrary"/>
		<rdfs:comment xml:lang="en">JavaLibrary implementing the javax.swing.plaf.basic package for J2SE 1.4</rdfs:comment>
		<rdfs:comment xml:lang="OWLManchester">platform:implementsInterface some JavaxSwingPlafBasicAPI</rdfs:comment>
	</owl:Class>
	<owl:Class rdf:about="#JavaxSwingPlafMetalClassLibrary">
		<rdfs:subClassOf rdf:resource="&j2se-1_3;JavaxSwingPlafMetalClassLibrary"/>
		<rdfs:comment xml:lang="en">JavaLibrary implementing the javax.swing.plaf.metal package for J2SE 1.4</rdfs:comment>
		<rdfs:comment xml:lang="OWLManchester">platform:implementsInterface some JavaxSwingPlafMetalAPI</rdfs:comment>
	</owl:Class>
	<owl:Class rdf:about="#JavaxSwingPlafMultiClassLibrary">
		<rdfs:subClassOf rdf:resource="&j2se-1_3;JavaxSwingPlafMultiClassLibrary"/>
		<rdfs:comment xml:lang="en">JavaLibrary implementing the javax.swing.plaf.multi package for J2SE 1.4</rdfs:comment>
		<rdfs:comment xml:lang="OWLManchester">platform:implementsInterface some JavaxSwingPlafMultiAPI</rdfs:comment>
	</owl:Class>
	<owl:Class rdf:about="#JavaxSwingEventClassLibrary">
		<rdfs:subClassOf rdf:resource="&j2se-1_3;JavaxSwingEventClassLibrary"/>
		<rdfs:comment xml:lang="en">JavaLibrary implementing the javax.swing.event package for J2SE 1.4</rdfs:comment>
		<rdfs:comment xml:lang="OWLManchester">platform:implementsInterface some JavaxSwingEventAPI</rdfs:comment>
	</owl:Class>
	<owl:Class rdf:about="#JavaxSwingBorderClassLibrary">
		<owl:equivalentClass rdf:resource="&j2se-1_3;JavaxSwingBorderClassLibrary"/>
		<rdfs:subClassOf rdf:resource="&java;JavaClassLibrary"/>
		<rdfs:comment xml:lang="en">JavaLibrary implementing the javax.swing.border package for J2SE 1.4</rdfs:comment>
		<rdfs:comment xml:lang="OWLManchester">platform:implementsInterface some JavaxSwingBorderAPI</rdfs:comment>
	</owl:Class>
	<owl:Class rdf:about="#JavaxSwingTextClassLibrary">
		<rdfs:subClassOf rdf:resource="&j2se-1_3;JavaxSwingTextClassLibrary"/>
		<rdfs:comment xml:lang="en">JavaLibrary implementing the javax.swing.text package for J2SE 1.4</rdfs:comment>
		<rdfs:comment xml:lang="OWLManchester">platform:implementsInterface some JavaxSwingTextAPI</rdfs:comment>
	</owl:Class>
	<owl:Class rdf:about="#JavaxSwingTextHtmlClassLibrary">
		<rdfs:subClassOf rdf:resource="&j2se-1_3;JavaxSwingTextHtmlClassLibrary"/>
		<rdfs:comment xml:lang="en">JavaLibrary implementing the javax.swing.text.html package for J2SE 1.4</rdfs:comment>
		<rdfs:comment xml:lang="OWLManchester">platform:implementsInterface some JavaxSwingTextHtmlAPI</rdfs:comment>
	</owl:Class>
	<owl:Class rdf:about="#JavaxSwingTextHtmlParserClassLibrary">
		<owl:equivalentClass rdf:resource="&j2se-1_3;JavaxSwingTextHtmlParserClassLibrary"/>
		<rdfs:subClassOf rdf:resource="&java;JavaClassLibrary"/>
		<rdfs:comment xml:lang="en">JavaLibrary implementing the javax.swing.text.html.parser package for J2SE 1.4</rdfs:comment>
		<rdfs:comment xml:lang="OWLManchester">platform:implementsInterface some JavaxSwingTextHtmlParserAPI</rdfs:comment>
	</owl:Class>
	<owl:Class rdf:about="#JavaxSwingTextRtfClassLibrary">
		<owl:equivalentClass rdf:resource="&j2se-1_3;JavaxSwingTextRtfClassLibrary"/>
		<rdfs:subClassOf rdf:resource="&java;JavaClassLibrary"/>
		<rdfs:comment xml:lang="en">JavaLibrary implementing the javax.swing.text.rtf package for J2SE 1.4</rdfs:comment>
		<rdfs:comment xml:lang="OWLManchester">platform:implementsInterface some JavaxSwingTextRtfAPI</rdfs:comment>
	</owl:Class>
	<owl:Class rdf:about="#JavaxSwingTableClassLibrary">
		<rdfs:subClassOf rdf:resource="&j2se-1_3;JavaxSwingTableClassLibrary"/>
		<rdfs:comment xml:lang="en">JavaLibrary implementing the javax.swing.table package for J2SE 1.4</rdfs:comment>
		<rdfs:comment xml:lang="OWLManchester">platform:implementsInterface some JavaxSwingTableAPI</rdfs:comment>
	</owl:Class>
	<owl:Class rdf:about="#JavaxSwingUndoClassLibrary">
		<rdfs:subClassOf rdf:resource="&j2se-1_3;JavaxSwingUndoClassLibrary"/>
		<rdfs:comment xml:lang="en">JavaLibrary implementing the javax.swing.undo package for J2SE 1.4</rdfs:comment>
		<rdfs:comment xml:lang="OWLManchester">platform:implementsInterface some JavaxSwingUndoAPI</rdfs:comment>
	</owl:Class>
	<owl:Class rdf:about="#JavaxSwingTreeClassLibrary">
		<rdfs:subClassOf rdf:resource="&j2se-1_3;JavaxSwingTreeClassLibrary"/>
		<rdfs:comment xml:lang="en">JavaLibrary implementing the javax.swing.tree package for J2SE 1.4</rdfs:comment>
		<rdfs:comment xml:lang="OWLManchester">platform:implementsInterface some JavaxSwingTreeAPI</rdfs:comment>
	</owl:Class>
	<owl:Class rdf:about="#JavaxSwingFilechooserClassLibrary">
		<rdfs:subClassOf rdf:resource="&j2se-1_3;JavaxSwingFilechooserClassLibrary"/>
		<rdfs:comment xml:lang="en">JavaLibrary implementing the javax.swing.filechooser package for J2SE 1.4</rdfs:comment>
		<rdfs:comment xml:lang="OWLManchester">platform:implementsInterface some JavaxSwingFilechooserAPI</rdfs:comment>
	</owl:Class>
	<owl:Class rdf:about="#JavaxSwingColorchooserClassLibrary">
		<rdfs:subClassOf rdf:resource="&j2se-1_3;JavaxSwingColorchooserClassLibrary"/>
		<rdfs:comment xml:lang="en">JavaLibrary implementing the javax.swing.colorchooser package for J2SE 1.4</rdfs:comment>
		<rdfs:comment xml:lang="OWLManchester">platform:implementsInterface some JavaxSwingColorchooserAPI</rdfs:comment>
	</owl:Class>
	<owl:Class rdf:about="#JavaxSoundSampledClassLibrary">
		<rdfs:subClassOf rdf:resource="&j2se-1_3;JavaxSoundSampledClassLibrary"/>
		<rdfs:comment xml:lang="en">JavaLibrary implementing the javax.sound.sampled package for J2SE 1.4</rdfs:comment>
		<rdfs:comment xml:lang="OWLManchester">platform:implementsInterface some JavaxSoundSampledAPI</rdfs:comment>
	</owl:Class>
	<owl:Class rdf:about="#JavaxSoundSampledSpiClassLibrary">
		<owl:equivalentClass rdf:resource="&j2se-1_3;JavaxSoundSampledSpiClassLibrary"/>
		<rdfs:subClassOf rdf:resource="&java;JavaClassLibrary"/>
		<rdfs:comment xml:lang="en">JavaLibrary implementing the javax.sound.sampled.spi package for J2SE 1.4</rdfs:comment>
		<rdfs:comment xml:lang="OWLManchester">platform:implementsInterface some JavaxSoundSampledSpiAPI</rdfs:comment>
	</owl:Class>
	<owl:Class rdf:about="#JavaxSoundMidiClassLibrary">
		<rdfs:subClassOf rdf:resource="&j2se-1_3;JavaxSoundMidiClassLibrary"/>
		<rdfs:comment xml:lang="en">JavaLibrary implementing the javax.sound.midi package for J2SE 1.4</rdfs:comment>
		<rdfs:comment xml:lang="OWLManchester">platform:implementsInterface some JavaxSoundMidiAPI</rdfs:comment>
	</owl:Class>
	<owl:Class rdf:about="#JavaxSoundMidiSpiClassLibrary">
		<owl:equivalentClass rdf:resource="&j2se-1_3;JavaxSoundMidiSpiClassLibrary"/>
		<rdfs:subClassOf rdf:resource="&java;JavaClassLibrary"/>
		<rdfs:comment xml:lang="en">JavaLibrary implementing the javax.sound.midi.spi package for J2SE 1.4</rdfs:comment>
		<rdfs:comment xml:lang="OWLManchester">platform:implementsInterface some JavaxSoundMidiSpiAPI</rdfs:comment>
	</owl:Class>
	<owl:Class rdf:about="#JavaxPrintClassLibrary">
		<rdfs:subClassOf rdf:resource="&java;JavaClassLibrary"/>
		<rdfs:comment xml:lang="en">JavaLibrary implementing the javax.print package for J2SE 1.4</rdfs:comment>
		<rdfs:comment xml:lang="OWLManchester">platform:implementsInterface some JavaxPrintAPI</rdfs:comment>
	</owl:Class>
	<owl:Class rdf:about="#JavaxPrintAttributeClassLibrary">
		<rdfs:subClassOf rdf:resource="&java;JavaClassLibrary"/>
		<rdfs:comment xml:lang="en">JavaLibrary implementing the javax.print.attribute package for J2SE 1.4</rdfs:comment>
		<rdfs:comment xml:lang="OWLManchester">platform:implementsInterface some JavaxPrintAttributeAPI</rdfs:comment>
	</owl:Class>
	<owl:Class rdf:about="#JavaxPrintAttributeStandardClassLibrary">
		<rdfs:subClassOf rdf:resource="&java;JavaClassLibrary"/>
		<rdfs:comment xml:lang="en">JavaLibrary implementing the javax.print.attribute.standard package for J2SE 1.4</rdfs:comment>
		<rdfs:comment xml:lang="OWLManchester">platform:implementsInterface some JavaxPrintAttributeStandardAPI</rdfs:comment>
	</owl:Class>
	<owl:Class rdf:about="#JavaxPrintEventClassLibrary">
		<rdfs:subClassOf rdf:resource="&java;JavaClassLibrary"/>
		<rdfs:comment xml:lang="en">JavaLibrary implementing the javax.print.event package for J2SE 1.4</rdfs:comment>
		<rdfs:comment xml:lang="OWLManchester">platform:implementsInterface some JavaxPrintEventAPI</rdfs:comment>
	</owl:Class>
	<owl:Class rdf:about="#JavaxSecurityAuthClassLibrary">
		<rdfs:subClassOf rdf:resource="&java;JavaClassLibrary"/>
		<rdfs:comment xml:lang="en">JavaLibrary implementing the javax.security.auth package for J2SE 1.4</rdfs:comment>
		<rdfs:comment xml:lang="OWLManchester">platform:implementsInterface some JavaxSecurityAuthAPI</rdfs:comment>
	</owl:Class>
	<owl:Class rdf:about="#JavaxSecurityAuthX500ClassLibrary">
		<rdfs:subClassOf rdf:resource="&j2me-pp-1_1;JavaxSecurityAuthX500ClassLibrary"/>
		<rdfs:comment xml:lang="en">JavaLibrary implementing the javax.security.auth.x500 package for J2SE 1.4</rdfs:comment>
		<rdfs:comment xml:lang="OWLManchester">platform:implementsInterface some JavaxSecurityAuthX500API</rdfs:comment>
	</owl:Class>
	<owl:Class rdf:about="#JavaxSecurityAuthCallbackClassLibrary">
		<rdfs:subClassOf rdf:resource="&java;JavaClassLibrary"/>
		<rdfs:comment xml:lang="en">JavaLibrary implementing the javax.security.auth.callback package for J2SE 1.4</rdfs:comment>
		<rdfs:comment xml:lang="OWLManchester">platform:implementsInterface some JavaxSecurityAuthCallbackAPI</rdfs:comment>
	</owl:Class>
	<owl:Class rdf:about="#JavaxSecurityAuthKerberosClassLibrary">
		<rdfs:subClassOf rdf:resource="&java;JavaClassLibrary"/>
		<rdfs:comment xml:lang="en">JavaLibrary implementing the javax.security.auth.kerberos package for J2SE 1.4</rdfs:comment>
		<rdfs:comment xml:lang="OWLManchester">platform:implementsInterface some JavaxSecurityAuthKerberosAPI</rdfs:comment>
	</owl:Class>
	<owl:Class rdf:about="#JavaxSecurityAuthLoginClassLibrary">
		<rdfs:subClassOf rdf:resource="&java;JavaClassLibrary"/>
		<rdfs:comment xml:lang="en">JavaLibrary implementing the javax.security.auth.login package for J2SE 1.4</rdfs:comment>
		<rdfs:comment xml:lang="OWLManchester">platform:implementsInterface some JavaxSecurityAuthLoginAPI</rdfs:comment>
	</owl:Class>
	<owl:Class rdf:about="#JavaxSecurityAuthSpiClassLibrary">
		<rdfs:subClassOf rdf:resource="&java;JavaClassLibrary"/>
		<rdfs:comment xml:lang="en">JavaLibrary implementing the javax.security.auth.spi package for J2SE 1.4</rdfs:comment>
		<rdfs:comment xml:lang="OWLManchester">platform:implementsInterface some JavaxSecurityAuthSpiAPI</rdfs:comment>
	</owl:Class>
	<owl:Class rdf:about="#JavaxSecurityCertClassLibrary">
		<rdfs:subClassOf rdf:resource="&java;JavaClassLibrary"/>
		<rdfs:comment xml:lang="en">JavaLibrary implementing the javax.security.cert package for J2SE 1.4</rdfs:comment>
		<rdfs:comment xml:lang="OWLManchester">platform:implementsInterface some JavaxSecurityCertAPI</rdfs:comment>
	</owl:Class>
	<owl:Class rdf:about="#JavaxNamingClassLibrary">
		<rdfs:subClassOf rdf:resource="&j2se-1_3;JavaxNamingClassLibrary"/>
		<rdfs:comment xml:lang="en">JavaLibrary implementing the javax.naming package for J2SE 1.4</rdfs:comment>
		<rdfs:comment xml:lang="OWLManchester">platform:implementsInterface some JavaxNamingAPI</rdfs:comment>
	</owl:Class>
	<owl:Class rdf:about="#JavaxNamingDirectoryClassLibrary">
		<rdfs:subClassOf rdf:resource="&j2se-1_3;JavaxNamingDirectoryClassLibrary"/>
		<rdfs:comment xml:lang="en">JavaLibrary implementing the javax.naming.directory package for J2SE 1.4</rdfs:comment>
		<rdfs:comment xml:lang="OWLManchester">platform:implementsInterface some JavaxNamingDirectoryAPI</rdfs:comment>
	</owl:Class>
	<owl:Class rdf:about="#JavaxNamingEventClassLibrary">
		<owl:equivalentClass rdf:resource="&j2se-1_3;JavaxNamingEventClassLibrary"/>
		<rdfs:subClassOf rdf:resource="&java;JavaClassLibrary"/>
		<rdfs:comment xml:lang="en">JavaLibrary implementing the javax.naming.event package for J2SE 1.4</rdfs:comment>
		<rdfs:comment xml:lang="OWLManchester">platform:implementsInterface some JavaxNamingEventAPI</rdfs:comment>
	</owl:Class>
	<owl:Class rdf:about="#JavaxNamingLdapClassLibrary">
		<rdfs:subClassOf rdf:resource="&j2se-1_3;JavaxNamingLdapClassLibrary"/>
		<rdfs:comment xml:lang="en">JavaLibrary implementing the javax.naming.ldap package for J2SE 1.4</rdfs:comment>
		<rdfs:comment xml:lang="OWLManchester">platform:implementsInterface some JavaxNamingLdapAPI</rdfs:comment>
	</owl:Class>
	<owl:Class rdf:about="#JavaxNamingSpiClassLibrary">
		<owl:equivalentClass rdf:resource="&j2se-1_3;JavaxNamingSpiClassLibrary"/>
		<rdfs:subClassOf rdf:resource="&java;JavaClassLibrary"/>
		<rdfs:comment xml:lang="en">JavaLibrary implementing the javax.naming.spi package for J2SE 1.4</rdfs:comment>
		<rdfs:comment xml:lang="OWLManchester">platform:implementsInterface some JavaxNamingSpiAPI</rdfs:comment>
	</owl:Class>
	<owl:Class rdf:about="#JavaxNetClassLibrary">
		<rdfs:subClassOf rdf:resource="&java;JavaClassLibrary"/>
		<rdfs:comment xml:lang="en">JavaLibrary implementing the javax.net package for J2SE 1.4</rdfs:comment>
		<rdfs:comment xml:lang="OWLManchester">platform:implementsInterface some JavaxNetAPI</rdfs:comment>
	</owl:Class>
	<owl:Class rdf:about="#JavaxNetSslClassLibrary">
		<rdfs:subClassOf rdf:resource="&java;JavaClassLibrary"/>
		<rdfs:comment xml:lang="en">JavaLibrary implementing the javax.net.ssl package for J2SE 1.4</rdfs:comment>
		<rdfs:comment xml:lang="OWLManchester">platform:implementsInterface some JavaxNetSslAPI</rdfs:comment>
	</owl:Class>
	<owl:Class rdf:about="#JavaxRmiClassLibrary">
		<owl:equivalentClass rdf:resource="&j2se-1_3;JavaxRmiClassLibrary"/>
		<rdfs:subClassOf rdf:resource="&java;JavaClassLibrary"/>
		<rdfs:comment xml:lang="en">JavaLibrary implementing the javax.rmi package for J2SE 1.4</rdfs:comment>
		<rdfs:comment xml:lang="OWLManchester">platform:implementsInterface some JavaxRmiAPI</rdfs:comment>
	</owl:Class>
	<owl:Class rdf:about="#JavaxRmiCORBAClassLibrary">
		<owl:equivalentClass rdf:resource="&j2se-1_3;JavaxRmiCORBAClassLibrary"/>
		<rdfs:subClassOf rdf:resource="&java;JavaClassLibrary"/>
		<rdfs:comment xml:lang="en">JavaLibrary implementing the javax.rmi.CORBA package for J2SE 1.4</rdfs:comment>
		<rdfs:comment xml:lang="OWLManchester">platform:implementsInterface some JavaxRmiCORBAAPI</rdfs:comment>
	</owl:Class>
	<owl:Class rdf:about="#JavaxCryptoClassLibrary">
		<rdfs:subClassOf rdf:resource="&java;JavaClassLibrary"/>
		<rdfs:comment xml:lang="en">JavaLibrary implementing the javax.crypto package for J2SE 1.4</rdfs:comment>
		<rdfs:comment xml:lang="OWLManchester">platform:implementsInterface some JavaxCryptoAPI</rdfs:comment>
	</owl:Class>
	<owl:Class rdf:about="#JavaxCryptoInterfacesClassLibrary">
		<rdfs:subClassOf rdf:resource="&java;JavaClassLibrary"/>
		<rdfs:comment xml:lang="en">JavaLibrary implementing the javax.crypto.interfaces package for J2SE 1.4</rdfs:comment>
		<rdfs:comment xml:lang="OWLManchester">platform:implementsInterface some JavaxCryptoInterfacesAPI</rdfs:comment>
	</owl:Class>
	<owl:Class rdf:about="#JavaxCryptoSpecClassLibrary">
		<rdfs:subClassOf rdf:resource="&java;JavaClassLibrary"/>
		<rdfs:comment xml:lang="en">JavaLibrary implementing the javax.crypto.spec package for J2SE 1.4</rdfs:comment>
		<rdfs:comment xml:lang="OWLManchester">platform:implementsInterface some JavaxCryptoSpecAPI</rdfs:comment>
	</owl:Class>
	<owl:Class rdf:about="#JavaxSqlClassLibrary">
		<rdfs:subClassOf rdf:resource="&java;JavaClassLibrary"/>
		<rdfs:comment xml:lang="en">JavaLibrary implementing the javax.sql package for J2SE 1.4</rdfs:comment>
		<rdfs:comment xml:lang="OWLManchester">platform:implementsInterface some JavaxSqlAPI</rdfs:comment>
	</owl:Class>
	<owl:Class rdf:about="#JavaxTransactionClassLibrary">
		<rdfs:subClassOf rdf:resource="&j2se-1_3;JavaxTransactionClassLibrary"/>
		<rdfs:comment xml:lang="en">JavaLibrary implementing the javax.transaction package for J2SE 1.4</rdfs:comment>
		<rdfs:comment xml:lang="OWLManchester">platform:implementsInterface some JavaxTransactionAPI</rdfs:comment>
	</owl:Class>
	<owl:Class rdf:about="#JavaxTransactionXaClassLibrary">
		<rdfs:subClassOf rdf:resource="&java;JavaClassLibrary"/>
		<rdfs:comment xml:lang="en">JavaLibrary implementing the javax.transaction.xa package for J2SE 1.4</rdfs:comment>
		<rdfs:comment xml:lang="OWLManchester">platform:implementsInterface some JavaxTransactionXaAPI</rdfs:comment>
	</owl:Class>
	<owl:Class rdf:about="#JavaxXmlParsersClassLibrary">
		<rdfs:subClassOf rdf:resource="&java;JavaClassLibrary"/>
		<rdfs:comment xml:lang="en">JavaLibrary implementing the javax.xml.parsers package for J2SE 1.4</rdfs:comment>
		<rdfs:comment xml:lang="OWLManchester">platform:implementsInterface some JavaxXmlParsersAPI</rdfs:comment>
	</owl:Class>
	<owl:Class rdf:about="#JavaxXmlTransformClassLibrary">
		<rdfs:subClassOf rdf:resource="&java;JavaClassLibrary"/>
		<rdfs:comment xml:lang="en">JavaLibrary implementing the javax.xml.transform package for J2SE 1.4</rdfs:comment>
		<rdfs:comment xml:lang="OWLManchester">platform:implementsInterface some JavaxXmlTransformAPI</rdfs:comment>
	</owl:Class>
	<owl:Class rdf:about="#JavaxXmlTransformDomClassLibrary">
		<rdfs:subClassOf rdf:resource="&java;JavaClassLibrary"/>
		<rdfs:comment xml:lang="en">JavaLibrary implementing the javax.xml.transform.dom package for J2SE 1.4</rdfs:comment>
		<rdfs:comment xml:lang="OWLManchester">platform:implementsInterface some JavaxXmlTransformDomAPI</rdfs:comment>
	</owl:Class>
	<owl:Class rdf:about="#JavaxXmlTransformSaxClassLibrary">
		<rdfs:subClassOf rdf:resource="&java;JavaClassLibrary"/>
		<rdfs:comment xml:lang="en">JavaLibrary implementing the javax.xml.transform.sax package for J2SE 1.4</rdfs:comment>
		<rdfs:comment xml:lang="OWLManchester">platform:implementsInterface some JavaxXmlTransformSaxAPI</rdfs:comment>
	</owl:Class>
	<owl:Class rdf:about="#JavaxXmlTransformStreamClassLibrary">
		<rdfs:subClassOf rdf:resource="&java;JavaClassLibrary"/>
		<rdfs:comment xml:lang="en">JavaLibrary implementing the javax.xml.transform.stream package for J2SE 1.4</rdfs:comment>
		<rdfs:comment xml:lang="OWLManchester">platform:implementsInterface some JavaxXmlTransformStreamAPI</rdfs:comment>
	</owl:Class>
	<owl:Class rdf:about="#OrgW3cDomClassLibrary">
		<rdfs:subClassOf rdf:resource="&java;JavaClassLibrary"/>
		<rdfs:comment xml:lang="en">JavaLibrary implementing the org.w3c.dom package for J2SE 1.4</rdfs:comment>
		<rdfs:comment xml:lang="OWLManchester">platform:implementsInterface some OrgW3cDomAPI</rdfs:comment>
	</owl:Class>
	<owl:Class rdf:about="#OrgW3cDomCssClassLibrary">
		<rdfs:subClassOf rdf:resource="&java;JavaClassLibrary"/>
		<rdfs:comment xml:lang="en">JavaLibrary implementing the org.w3c.dom.css package for J2SE 1.4</rdfs:comment>
		<rdfs:comment xml:lang="OWLManchester">platform:implementsInterface some OrgW3cDomCssAPI</rdfs:comment>
	</owl:Class>
	<owl:Class rdf:about="#OrgW3cDomStylesheetsClassLibrary">
		<rdfs:subClassOf rdf:resource="&java;JavaClassLibrary"/>
		<rdfs:comment xml:lang="en">JavaLibrary implementing the org.w3c.dom.stylesheets package for J2SE 1.4</rdfs:comment>
		<rdfs:comment xml:lang="OWLManchester">platform:implementsInterface some OrgW3cDomStylesheetsAPI</rdfs:comment>
	</owl:Class>
	<owl:Class rdf:about="#OrgW3cDomViewsClassLibrary">
		<rdfs:subClassOf rdf:resource="&java;JavaClassLibrary"/>
		<rdfs:comment xml:lang="en">JavaLibrary implementing the org.w3c.dom.views package for J2SE 1.4</rdfs:comment>
		<rdfs:comment xml:lang="OWLManchester">platform:implementsInterface some OrgW3cDomViewsAPI</rdfs:comment>
	</owl:Class>
	<owl:Class rdf:about="#OrgW3cDomEventsClassLibrary">
		<rdfs:subClassOf rdf:resource="&java;JavaClassLibrary"/>
		<rdfs:comment xml:lang="en">JavaLibrary implementing the org.w3c.dom.events package for J2SE 1.4</rdfs:comment>
		<rdfs:comment xml:lang="OWLManchester">platform:implementsInterface some OrgW3cDomEventsAPI</rdfs:comment>
	</owl:Class>
	<owl:Class rdf:about="#OrgW3cDomHtmlClassLibrary">
		<rdfs:subClassOf rdf:resource="&java;JavaClassLibrary"/>
		<rdfs:comment xml:lang="en">JavaLibrary implementing the org.w3c.dom.html package for J2SE 1.4</rdfs:comment>
		<rdfs:comment xml:lang="OWLManchester">platform:implementsInterface some OrgW3cDomHtmlAPI</rdfs:comment>
	</owl:Class>
	<owl:Class rdf:about="#OrgW3cDomTraversalClassLibrary">
		<rdfs:subClassOf rdf:resource="&java;JavaClassLibrary"/>
		<rdfs:comment xml:lang="en">JavaLibrary implementing the org.w3c.dom.traversal package for J2SE 1.4</rdfs:comment>
		<rdfs:comment xml:lang="OWLManchester">platform:implementsInterface some OrgW3cDomTraversalAPI</rdfs:comment>
	</owl:Class>
	<owl:Class rdf:about="#OrgOmgCORBA_2_3ClassLibrary">
		<owl:equivalentClass rdf:resource="&j2se-1_3;OrgOmgCORBA_2_3ClassLibrary"/>
		<rdfs:subClassOf rdf:resource="&java;JavaClassLibrary"/>
		<rdfs:comment xml:lang="en">JavaLibrary implementing the org.omg.CORBA_2_3 package for J2SE 1.4</rdfs:comment>
		<rdfs:comment xml:lang="OWLManchester">platform:implementsInterface some OrgOmgCORBA_2_3API</rdfs:comment>
	</owl:Class>
	<owl:Class rdf:about="#OrgOmgCORBA_2_3PortableClassLibrary">
		<rdfs:subClassOf rdf:resource="&java;JavaClassLibrary"/>
		<rdfs:comment xml:lang="en">JavaLibrary implementing the org.omg.CORBA_2_3.portable package for J2SE 1.4</rdfs:comment>
		<rdfs:comment xml:lang="OWLManchester">platform:implementsInterface some OrgOmgCORBA_2_3PortableAPI</rdfs:comment>
	</owl:Class>
	<owl:Class rdf:about="#OrgOmgCORBAClassLibrary">
		<rdfs:subClassOf rdf:resource="&java;JavaClassLibrary"/>
		<rdfs:comment xml:lang="en">JavaLibrary implementing the org.omg.CORBA package for J2SE 1.4</rdfs:comment>
		<rdfs:comment xml:lang="OWLManchester">platform:implementsInterface some OrgOmgCORBAAPI</rdfs:comment>
	</owl:Class>
	<owl:Class rdf:about="#OrgOmgCORBAPortableClassLibrary">
		<rdfs:subClassOf rdf:resource="&java;JavaClassLibrary"/>
		<rdfs:comment xml:lang="en">JavaLibrary implementing the org.omg.CORBA.portable package for J2SE 1.4</rdfs:comment>
		<rdfs:comment xml:lang="OWLManchester">platform:implementsInterface some OrgOmgCORBAPortableAPI</rdfs:comment>
	</owl:Class>
	<owl:Class rdf:about="#OrgOmgCORBADynAnyPackageClassLibrary">
		<rdfs:subClassOf rdf:resource="&j2se-1_3;OrgOmgCORBADynAnyPackageClassLibrary"/>
		<rdfs:comment xml:lang="en">JavaLibrary implementing the org.omg.CORBA.DynAnyPackage package for J2SE 1.4</rdfs:comment>
		<rdfs:comment xml:lang="OWLManchester">platform:implementsInterface some OrgOmgCORBADynAnyPackageAPI</rdfs:comment>
	</owl:Class>
	<owl:Class rdf:about="#OrgOmgCORBAORBPackageClassLibrary">
		<rdfs:subClassOf rdf:resource="&j2se-1_3;OrgOmgCORBAORBPackageClassLibrary"/>
		<rdfs:comment xml:lang="en">JavaLibrary implementing the org.omg.CORBA.ORBPackage package for J2SE 1.4</rdfs:comment>
		<rdfs:comment xml:lang="OWLManchester">platform:implementsInterface some OrgOmgCORBAORBPackageAPI</rdfs:comment>
	</owl:Class>
	<owl:Class rdf:about="#OrgOmgCORBATypeCodePackageClassLibrary">
		<rdfs:subClassOf rdf:resource="&j2se-1_3;OrgOmgCORBATypeCodePackageClassLibrary"/>
		<rdfs:comment xml:lang="en">JavaLibrary implementing the org.omg.CORBA.TypeCodePackage package for J2SE 1.4</rdfs:comment>
		<rdfs:comment xml:lang="OWLManchester">platform:implementsInterface some OrgOmgCORBATypeCodePackageAPI</rdfs:comment>
	</owl:Class>
	<owl:Class rdf:about="#OrgOmgSendingContextClassLibrary">
		<owl:equivalentClass rdf:resource="&j2se-1_3;OrgOmgSendingContextClassLibrary"/>
		<rdfs:subClassOf rdf:resource="&java;JavaClassLibrary"/>
		<rdfs:comment xml:lang="en">JavaLibrary implementing the org.omg.SendingContext package for J2SE 1.4</rdfs:comment>
		<rdfs:comment xml:lang="OWLManchester">platform:implementsInterface some OrgOmgSendingContextAPI</rdfs:comment>
	</owl:Class>
	<owl:Class rdf:about="#OrgOmgCosNamingClassLibrary">
		<rdfs:subClassOf rdf:resource="&java;JavaClassLibrary"/>
		<rdfs:comment xml:lang="en">JavaLibrary implementing the org.omg.CosNaming package for J2SE 1.4</rdfs:comment>
		<rdfs:comment xml:lang="OWLManchester">platform:implementsInterface some OrgOmgCosNamingAPI</rdfs:comment>
	</owl:Class>
	<owl:Class rdf:about="#OrgOmgCosNamingNamingContextExtPackageClassLibrary">
		<rdfs:subClassOf rdf:resource="&java;JavaClassLibrary"/>
		<rdfs:comment xml:lang="en">JavaLibrary implementing the org.omg.CosNaming.NamingContextExtPackage package for J2SE 1.4</rdfs:comment>
		<rdfs:comment xml:lang="OWLManchester">platform:implementsInterface some OrgOmgCosNamingNamingContextExtPackageAPI</rdfs:comment>
	</owl:Class>
	<owl:Class rdf:about="#OrgOmgCosNamingNamingContextPackageClassLibrary">
		<rdfs:subClassOf rdf:resource="&java;JavaClassLibrary"/>
		<rdfs:comment xml:lang="en">JavaLibrary implementing the org.omg.CosNaming.NamingContextPackage package for J2SE 1.4</rdfs:comment>
		<rdfs:comment xml:lang="OWLManchester">platform:implementsInterface some OrgOmgCosNamingNamingContextPackageAPI</rdfs:comment>
	</owl:Class>
	<owl:Class rdf:about="#OrgOmgPortableServerClassLibrary">
		<rdfs:subClassOf rdf:resource="&java;JavaClassLibrary"/>
		<rdfs:comment xml:lang="en">JavaLibrary implementing the org.omg.PortableServer package for J2SE 1.4</rdfs:comment>
		<rdfs:comment xml:lang="OWLManchester">platform:implementsInterface some OrgOmgPortableServerAPI</rdfs:comment>
	</owl:Class>
	<owl:Class rdf:about="#OrgOmgPortableServerCurrentPackageClassLibrary">
		<rdfs:subClassOf rdf:resource="&java;JavaClassLibrary"/>
		<rdfs:comment xml:lang="en">JavaLibrary implementing the org.omg.PortableServer.CurrentPackage package for J2SE 1.4</rdfs:comment>
		<rdfs:comment xml:lang="OWLManchester">platform:implementsInterface some OrgOmgPortableServerCurrentPackageAPI</rdfs:comment>
	</owl:Class>
	<owl:Class rdf:about="#OrgOmgPortableServerPOAManagerPackageClassLibrary">
		<rdfs:subClassOf rdf:resource="&java;JavaClassLibrary"/>
		<rdfs:comment xml:lang="en">JavaLibrary implementing the org.omg.PortableServer.POAManagerPackage package for J2SE 1.4</rdfs:comment>
		<rdfs:comment xml:lang="OWLManchester">platform:implementsInterface some OrgOmgPortableServerPOAManagerPackageAPI</rdfs:comment>
	</owl:Class>
	<owl:Class rdf:about="#OrgOmgPortableServerPOAPackageClassLibrary">
		<rdfs:subClassOf rdf:resource="&java;JavaClassLibrary"/>
		<rdfs:comment xml:lang="en">JavaLibrary implementing the org.omg.PortableServer.POAPackage package for J2SE 1.4</rdfs:comment>
		<rdfs:comment xml:lang="OWLManchester">platform:implementsInterface some OrgOmgPortableServerPOAPackageAPI</rdfs:comment>
	</owl:Class>
	<owl:Class rdf:about="#OrgOmgPortableServerPortableClassLibrary">
		<rdfs:subClassOf rdf:resource="&java;JavaClassLibrary"/>
		<rdfs:comment xml:lang="en">JavaLibrary implementing the org.omg.PortableServer.portable package for J2SE 1.4</rdfs:comment>
		<rdfs:comment xml:lang="OWLManchester">platform:implementsInterface some OrgOmgPortableServerPortableAPI</rdfs:comment>
	</owl:Class>
	<owl:Class rdf:about="#OrgOmgPortableServerServantLocatorPackageClassLibrary">
		<rdfs:subClassOf rdf:resource="&java;JavaClassLibrary"/>
		<rdfs:comment xml:lang="en">JavaLibrary implementing the org.omg.PortableServer.ServantLocatorPackage package for J2SE 1.4</rdfs:comment>
		<rdfs:comment xml:lang="OWLManchester">platform:implementsInterface some OrgOmgPortableServerServantLocatorPackageAPI</rdfs:comment>
	</owl:Class>
	<owl:Class rdf:about="#OrgOmgDynamicClassLibrary">
		<rdfs:subClassOf rdf:resource="&java;JavaClassLibrary"/>
		<rdfs:comment xml:lang="en">JavaLibrary implementing the org.omg.Dynamic package for J2SE 1.4</rdfs:comment>
		<rdfs:comment xml:lang="OWLManchester">platform:implementsInterface some OrgOmgDynamicAPI</rdfs:comment>
	</owl:Class>
	<owl:Class rdf:about="#OrgOmgDynamicAnyClassLibrary">
		<rdfs:subClassOf rdf:resource="&java;JavaClassLibrary"/>
		<rdfs:comment xml:lang="en">JavaLibrary implementing the org.omg.DynamicAny package for J2SE 1.4</rdfs:comment>
		<rdfs:comment xml:lang="OWLManchester">platform:implementsInterface some OrgOmgDynamicAnyAPI</rdfs:comment>
	</owl:Class>
	<owl:Class rdf:about="#OrgOmgDynamicAnyDynAnyFactoryPackageClassLibrary">
		<rdfs:subClassOf rdf:resource="&java;JavaClassLibrary"/>
		<rdfs:comment xml:lang="en">JavaLibrary implementing the org.omg.DynamicAny.DynAnyFactoryPackage package for J2SE 1.4</rdfs:comment>
		<rdfs:comment xml:lang="OWLManchester">platform:implementsInterface some OrgOmgDynamicAnyDynAnyFactoryPackageAPI</rdfs:comment>
	</owl:Class>
	<owl:Class rdf:about="#OrgOmgDynamicAnyDynAnyPackageClassLibrary">
		<rdfs:subClassOf rdf:resource="&java;JavaClassLibrary"/>
		<rdfs:comment xml:lang="en">JavaLibrary implementing the org.omg.DynamicAny.DynAnyPackage package for J2SE 1.4</rdfs:comment>
		<rdfs:comment xml:lang="OWLManchester">platform:implementsInterface some OrgOmgDynamicAnyDynAnyPackageAPI</rdfs:comment>
	</owl:Class>
	<owl:Class rdf:about="#OrgOmgIOPClassLibrary">
		<rdfs:subClassOf rdf:resource="&java;JavaClassLibrary"/>
		<rdfs:comment xml:lang="en">JavaLibrary implementing the org.omg.IOP package for J2SE 1.4</rdfs:comment>
		<rdfs:comment xml:lang="OWLManchester">platform:implementsInterface some OrgOmgIOPAPI</rdfs:comment>
	</owl:Class>
	<owl:Class rdf:about="#OrgOmgIOPCodecFactoryPackageClassLibrary">
		<rdfs:subClassOf rdf:resource="&java;JavaClassLibrary"/>
		<rdfs:comment xml:lang="en">JavaLibrary implementing the org.omg.IOP.CodecFactoryPackage package for J2SE 1.4</rdfs:comment>
		<rdfs:comment xml:lang="OWLManchester">platform:implementsInterface some OrgOmgIOPCodecFactoryPackageAPI</rdfs:comment>
	</owl:Class>
	<owl:Class rdf:about="#OrgOmgIOPCodecPackageClassLibrary">
		<rdfs:subClassOf rdf:resource="&java;JavaClassLibrary"/>
		<rdfs:comment xml:lang="en">JavaLibrary implementing the org.omg.IOP.CodecPackage package for J2SE 1.4</rdfs:comment>
		<rdfs:comment xml:lang="OWLManchester">platform:implementsInterface some OrgOmgIOPCodecPackageAPI</rdfs:comment>
	</owl:Class>
	<owl:Class rdf:about="#OrgOmgMessagingClassLibrary">
		<rdfs:subClassOf rdf:resource="&java;JavaClassLibrary"/>
		<rdfs:comment xml:lang="en">JavaLibrary implementing the org.omg.Messaging package for J2SE 1.4</rdfs:comment>
		<rdfs:comment xml:lang="OWLManchester">platform:implementsInterface some OrgOmgMessagingAPI</rdfs:comment>
	</owl:Class>
	<owl:Class rdf:about="#OrgOmgPortableInterceptorClassLibrary">
		<rdfs:subClassOf rdf:resource="&java;JavaClassLibrary"/>
		<rdfs:comment xml:lang="en">JavaLibrary implementing the org.omg.PortableInterceptor package for J2SE 1.4</rdfs:comment>
		<rdfs:comment xml:lang="OWLManchester">platform:implementsInterface some OrgOmgPortableInterceptorAPI</rdfs:comment>
	</owl:Class>
	<owl:Class rdf:about="#OrgOmgPortableInterceptorORBInitInfoPackageClassLibrary">
		<rdfs:subClassOf rdf:resource="&java;JavaClassLibrary"/>
		<rdfs:comment xml:lang="en">JavaLibrary implementing the org.omg.PortableInterceptor.ORBInitInfoPackage package for J2SE 1.4</rdfs:comment>
		<rdfs:comment xml:lang="OWLManchester">platform:implementsInterface some OrgOmgPortableInterceptorORBInitInfoPackageAPI</rdfs:comment>
	</owl:Class>
	<owl:Class rdf:about="#OrgOmgStubJavaRmiClassLibrary">
		<owl:equivalentClass rdf:resource="&j2se-1_3;OrgOmgStubJavaRmiClassLibrary"/>
		<rdfs:subClassOf rdf:resource="&java;JavaClassLibrary"/>
		<rdfs:comment xml:lang="en">JavaLibrary implementing the org.omg.stub.java.rmi package for J2SE 1.4</rdfs:comment>
		<rdfs:comment xml:lang="OWLManchester">platform:implementsInterface some OrgOmgStubJavaRmiAPI</rdfs:comment>
	</owl:Class>
	<owl:Class rdf:about="#OrgXmlSaxClassLibrary">
		<rdfs:subClassOf rdf:resource="&java;JavaClassLibrary"/>
		<rdfs:comment xml:lang="en">JavaLibrary implementing the org.xml.sax package for J2SE 1.4</rdfs:comment>
		<rdfs:comment xml:lang="OWLManchester">platform:implementsInterface some OrgXmlSaxAPI</rdfs:comment>
	</owl:Class>
	<owl:Class rdf:about="#OrgXmlSaxHelpersClassLibrary">
		<rdfs:subClassOf rdf:resource="&java;JavaClassLibrary"/>
		<rdfs:comment xml:lang="en">JavaLibrary implementing the org.xml.sax.helpers package for J2SE 1.4</rdfs:comment>
		<rdfs:comment xml:lang="OWLManchester">platform:implementsInterface some OrgXmlSaxHelpersAPI</rdfs:comment>
	</owl:Class>
	<owl:Class rdf:about="#OrgXmlSaxExtClassLibrary">
		<rdfs:subClassOf rdf:resource="&java;JavaClassLibrary"/>
		<rdfs:comment xml:lang="en">JavaLibrary implementing the org.xml.sax.ext package for J2SE 1.4</rdfs:comment>
		<rdfs:comment xml:lang="OWLManchester">platform:implementsInterface some OrgXmlSaxExtAPI</rdfs:comment>
	</owl:Class>
	<owl:Class rdf:about="#OrgIetfJgssClassLibrary">
		<rdfs:subClassOf rdf:resource="&java;JavaClassLibrary"/>
		<rdfs:comment xml:lang="en">JavaLibrary implementing the org.ietf.jgss package for J2SE 1.4</rdfs:comment>
		<rdfs:comment xml:lang="OWLManchester">platform:implementsInterface some OrgIetfJgssAPI</rdfs:comment>
	</owl:Class>
</rdf:RDF>
