<?xml version="1.0" encoding="ISO-8859-1"?>
<!DOCTYPE rdf:RDF [
	<!ENTITY isa "http://soft.vub.ac.be/platformkit/2010/1/isa.owl#">
	<!ENTITY platform "http://soft.vub.ac.be/platformkit/2010/1/platform.owl#">
	<!ENTITY java "http://soft.vub.ac.be/platformkit/2010/1/java.owl#">
	<!ENTITY xsd "http://www.w3.org/2001/XMLSchema#">
	<!ENTITY rdf "http://www.w3.org/1999/02/22-rdf-syntax-ns#">
	<!ENTITY owl "http://www.w3.org/2002/07/owl#">
	<!ENTITY rdfs "http://www.w3.org/2000/01/rdf-schema#">
]>
<rdf:RDF
	 xmlns="http://soft.vub.ac.be/platformkit/2010/1/swt-3_0.owl#"
	 xml:base="http://soft.vub.ac.be/platformkit/2010/1/swt-3_0.owl"
	 xmlns:isa="&isa;"
	 xmlns:platform="&platform;"
	 xmlns:java="&java;"
	 xmlns:xsd="&xsd;"
	 xmlns:rdf="&rdf;"
	 xmlns:owl="&owl;"
	 xmlns:rdfs="&rdfs;"
>

	<owl:Ontology rdf:about="">
		<owl:versionInfo>$Id$</owl:versionInfo>
		<owl:imports rdf:resource="http://soft.vub.ac.be/platformkit/2010/1/platform.owl"/>
		<owl:imports rdf:resource="http://soft.vub.ac.be/platformkit/2010/1/java.owl"/>
		<rdfs:comment xml:lang="en">Generated by [UML2ToSimplifiedPackageAPIOntology.atl 8080 2010-03-18 10:46:40Z dwagelaa], [UML2ToPackageAPIOntology.atl 8082 2010-03-18 21:11:00Z dwagelaa], [UML2ToAPIOntology.atl 8086 2010-03-19 09:49:17Z dwagelaa], and [UML2Comparison.atl 8086 2010-03-19 09:49:17Z dwagelaa]</rdfs:comment>
		<rdfs:comment>Dennis Wagelaar &lt;dennis.wagelaar@vub.ac.be&gt;</rdfs:comment>
		<rdfs:comment xml:lang="en">&#169; 2010, Vrije Universiteit Brussel. All rights reserved.</rdfs:comment>
		<rdfs:label xml:lang="en">SWT 3.0</rdfs:label>
	</owl:Ontology>
	<owl:Class rdf:about="#SWT3_0API">
		<rdfs:subClassOf rdf:resource="#OrgEclipseSwtAPI"/>
		<rdfs:subClassOf rdf:resource="#OrgEclipseSwtAccessibilityAPI"/>
		<rdfs:subClassOf rdf:resource="#OrgEclipseSwtWidgetsAPI"/>
		<rdfs:subClassOf rdf:resource="#OrgEclipseSwtAwtAPI"/>
		<rdfs:subClassOf rdf:resource="#OrgEclipseSwtBrowserAPI"/>
		<rdfs:subClassOf rdf:resource="#OrgEclipseSwtEventsAPI"/>
		<rdfs:subClassOf rdf:resource="#OrgEclipseSwtGraphicsAPI"/>
		<rdfs:subClassOf rdf:resource="#OrgEclipseSwtCustomAPI"/>
		<rdfs:subClassOf rdf:resource="#OrgEclipseSwtPrintingAPI"/>
		<rdfs:subClassOf rdf:resource="#OrgEclipseSwtDndAPI"/>
		<rdfs:subClassOf rdf:resource="#OrgEclipseSwtLayoutAPI"/>
		<rdfs:subClassOf rdf:resource="#OrgEclipseSwtProgramAPI"/>
		<rdfs:comment xml:lang="en">SWT 3.0 API</rdfs:comment>
		<rdfs:comment xml:lang="OWLManchester">platform:comprisesInterfacePart some OrgEclipseSwt and platform:comprisesInterfacePart some OrgEclipseSwtAccessibility and platform:comprisesInterfacePart some OrgEclipseSwtWidgets and platform:comprisesInterfacePart some OrgEclipseSwtAwt and platform:comprisesInterfacePart some OrgEclipseSwtBrowser and platform:comprisesInterfacePart some OrgEclipseSwtEvents and platform:comprisesInterfacePart some OrgEclipseSwtGraphics and platform:comprisesInterfacePart some OrgEclipseSwtCustom and platform:comprisesInterfacePart some OrgEclipseSwtPrinting and platform:comprisesInterfacePart some OrgEclipseSwtDnd and platform:comprisesInterfacePart some OrgEclipseSwtLayout and platform:comprisesInterfacePart some OrgEclipseSwtProgram</rdfs:comment>
	</owl:Class>
	<owl:Class rdf:about="#SWT3_0ClassLibrary">
		<rdfs:subClassOf rdf:resource="#OrgEclipseSwtClassLibrary"/>
		<rdfs:subClassOf rdf:resource="#OrgEclipseSwtAccessibilityClassLibrary"/>
		<rdfs:subClassOf rdf:resource="#OrgEclipseSwtWidgetsClassLibrary"/>
		<rdfs:subClassOf rdf:resource="#OrgEclipseSwtAwtClassLibrary"/>
		<rdfs:subClassOf rdf:resource="#OrgEclipseSwtBrowserClassLibrary"/>
		<rdfs:subClassOf rdf:resource="#OrgEclipseSwtEventsClassLibrary"/>
		<rdfs:subClassOf rdf:resource="#OrgEclipseSwtGraphicsClassLibrary"/>
		<rdfs:subClassOf rdf:resource="#OrgEclipseSwtCustomClassLibrary"/>
		<rdfs:subClassOf rdf:resource="#OrgEclipseSwtPrintingClassLibrary"/>
		<rdfs:subClassOf rdf:resource="#OrgEclipseSwtDndClassLibrary"/>
		<rdfs:subClassOf rdf:resource="#OrgEclipseSwtLayoutClassLibrary"/>
		<rdfs:subClassOf rdf:resource="#OrgEclipseSwtProgramClassLibrary"/>
		<rdfs:comment xml:lang="en">Java class library implementing the SWT 3.0 API</rdfs:comment>
		<rdfs:comment xml:lang="OWLManchester">platform:implementsInterface some SWT3_0API</rdfs:comment>
	</owl:Class>
	<SWT3_0API rdf:about="#theSWT3_0API">
		<platform:comprisesInterfacePart rdf:resource="#theOrgEclipseSwtProgramPart"/>
		<platform:comprisesInterfacePart rdf:resource="#theOrgEclipseSwtLayoutPart"/>
		<platform:comprisesInterfacePart rdf:resource="#theOrgEclipseSwtDndPart"/>
		<platform:comprisesInterfacePart rdf:resource="#theOrgEclipseSwtPrintingPart"/>
		<platform:comprisesInterfacePart rdf:resource="#theOrgEclipseSwtCustomPart"/>
		<platform:comprisesInterfacePart rdf:resource="#theOrgEclipseSwtGraphicsPart"/>
		<platform:comprisesInterfacePart rdf:resource="#theOrgEclipseSwtEventsPart"/>
		<platform:comprisesInterfacePart rdf:resource="#theOrgEclipseSwtBrowserPart"/>
		<platform:comprisesInterfacePart rdf:resource="#theOrgEclipseSwtAwtPart"/>
		<platform:comprisesInterfacePart rdf:resource="#theOrgEclipseSwtWidgetsPart"/>
		<platform:comprisesInterfacePart rdf:resource="#theOrgEclipseSwtAccessibilityPart"/>
		<platform:comprisesInterfacePart rdf:resource="#theOrgEclipseSwtPart"/>
	</SWT3_0API>
	<owl:Class rdf:about="#OrgEclipseSwt">
		<rdfs:subClassOf rdf:resource="&java;JavaAPIPart"/>
		<rdfs:comment xml:lang="en">Java API part implementing the org.eclipse.swt package for SWT 3.0</rdfs:comment>
	</owl:Class>
	<owl:Class rdf:about="#OrgEclipseSwtAccessibility">
		<rdfs:subClassOf rdf:resource="&java;JavaAPIPart"/>
		<rdfs:seeAlso rdf:resource="#OrgEclipseSwtWidgets"/>
		<rdfs:comment xml:lang="en">Java API part implementing the org.eclipse.swt.accessibility package for SWT 3.0</rdfs:comment>
	</owl:Class>
	<owl:Class rdf:about="#OrgEclipseSwtWidgets">
		<rdfs:subClassOf rdf:resource="&java;JavaAPIPart"/>
		<rdfs:seeAlso rdf:resource="#OrgEclipseSwtAccessibility"/>
		<rdfs:seeAlso rdf:resource="#OrgEclipseSwtGraphics"/>
		<rdfs:seeAlso rdf:resource="#OrgEclipseSwtEvents"/>
		<rdfs:comment xml:lang="en">Java API part implementing the org.eclipse.swt.widgets package for SWT 3.0</rdfs:comment>
	</owl:Class>
	<owl:Class rdf:about="#OrgEclipseSwtAwt">
		<rdfs:subClassOf rdf:resource="&java;JavaAPIPart"/>
		<rdfs:seeAlso rdf:resource="#OrgEclipseSwtWidgets"/>
		<rdfs:comment xml:lang="en">Java API part implementing the org.eclipse.swt.awt package for SWT 3.0</rdfs:comment>
	</owl:Class>
	<owl:Class rdf:about="#OrgEclipseSwtBrowser">
		<rdfs:subClassOf rdf:resource="&java;JavaAPIPart"/>
		<rdfs:seeAlso rdf:resource="#OrgEclipseSwtWidgets"/>
		<rdfs:seeAlso rdf:resource="#OrgEclipseSwtGraphics"/>
		<rdfs:seeAlso rdf:resource="#OrgEclipseSwtEvents"/>
		<rdfs:comment xml:lang="en">Java API part implementing the org.eclipse.swt.browser package for SWT 3.0</rdfs:comment>
	</owl:Class>
	<owl:Class rdf:about="#OrgEclipseSwtEvents">
		<rdfs:subClassOf rdf:resource="&java;JavaAPIPart"/>
		<rdfs:seeAlso rdf:resource="#OrgEclipseSwtWidgets"/>
		<rdfs:seeAlso rdf:resource="#OrgEclipseSwtGraphics"/>
		<rdfs:comment xml:lang="en">Java API part implementing the org.eclipse.swt.events package for SWT 3.0</rdfs:comment>
	</owl:Class>
	<owl:Class rdf:about="#OrgEclipseSwtGraphics">
		<rdfs:subClassOf rdf:resource="&java;JavaAPIPart"/>
		<rdfs:comment xml:lang="en">Java API part implementing the org.eclipse.swt.graphics package for SWT 3.0</rdfs:comment>
	</owl:Class>
	<owl:Class rdf:about="#OrgEclipseSwtCustom">
		<rdfs:subClassOf rdf:resource="&java;JavaAPIPart"/>
		<rdfs:seeAlso rdf:resource="#OrgEclipseSwtGraphics"/>
		<rdfs:seeAlso rdf:resource="#OrgEclipseSwtPrinting"/>
		<rdfs:seeAlso rdf:resource="#OrgEclipseSwtEvents"/>
		<rdfs:seeAlso rdf:resource="#OrgEclipseSwtWidgets"/>
		<rdfs:comment xml:lang="en">Java API part implementing the org.eclipse.swt.custom package for SWT 3.0</rdfs:comment>
	</owl:Class>
	<owl:Class rdf:about="#OrgEclipseSwtPrinting">
		<rdfs:subClassOf rdf:resource="&java;JavaAPIPart"/>
		<rdfs:seeAlso rdf:resource="#OrgEclipseSwtWidgets"/>
		<rdfs:seeAlso rdf:resource="#OrgEclipseSwtGraphics"/>
		<rdfs:comment xml:lang="en">Java API part implementing the org.eclipse.swt.printing package for SWT 3.0</rdfs:comment>
	</owl:Class>
	<owl:Class rdf:about="#OrgEclipseSwtDnd">
		<rdfs:subClassOf rdf:resource="&java;JavaAPIPart"/>
		<rdfs:seeAlso rdf:resource="#OrgEclipseSwtWidgets"/>
		<rdfs:seeAlso rdf:resource="#OrgEclipseSwtEvents"/>
		<rdfs:comment xml:lang="en">Java API part implementing the org.eclipse.swt.dnd package for SWT 3.0</rdfs:comment>
	</owl:Class>
	<owl:Class rdf:about="#OrgEclipseSwtLayout">
		<rdfs:subClassOf rdf:resource="&java;JavaAPIPart"/>
		<rdfs:seeAlso rdf:resource="#OrgEclipseSwtGraphics"/>
		<rdfs:seeAlso rdf:resource="#OrgEclipseSwtWidgets"/>
		<rdfs:comment xml:lang="en">Java API part implementing the org.eclipse.swt.layout package for SWT 3.0</rdfs:comment>
	</owl:Class>
	<owl:Class rdf:about="#OrgEclipseSwtProgram">
		<rdfs:subClassOf rdf:resource="&java;JavaAPIPart"/>
		<rdfs:seeAlso rdf:resource="#OrgEclipseSwtGraphics"/>
		<rdfs:comment xml:lang="en">Java API part implementing the org.eclipse.swt.program package for SWT 3.0</rdfs:comment>
	</owl:Class>
	<owl:Class rdf:about="#OrgEclipseSwtAPI">
		<rdfs:subClassOf rdf:resource="&java;JavaAPI"/>
		<rdfs:comment xml:lang="en">JavaLibrary implementing the org.eclipse.swt package for SWT 3.0</rdfs:comment>
		<rdfs:comment xml:lang="OWLManchester">platform:comprisesInterfacePart some OrgEclipseSwt</rdfs:comment>
	</owl:Class>
	<owl:Class rdf:about="#OrgEclipseSwtAccessibilityAPI">
		<rdfs:subClassOf rdf:resource="&java;JavaAPI"/>
		<rdfs:comment xml:lang="en">JavaLibrary implementing the org.eclipse.swt.accessibility package for SWT 3.0</rdfs:comment>
		<rdfs:comment xml:lang="OWLManchester">platform:comprisesInterfacePart some OrgEclipseSwtAccessibility</rdfs:comment>
	</owl:Class>
	<owl:Class rdf:about="#OrgEclipseSwtWidgetsAPI">
		<rdfs:subClassOf rdf:resource="&java;JavaAPI"/>
		<rdfs:comment xml:lang="en">JavaLibrary implementing the org.eclipse.swt.widgets package for SWT 3.0</rdfs:comment>
		<rdfs:comment xml:lang="OWLManchester">platform:comprisesInterfacePart some OrgEclipseSwtWidgets</rdfs:comment>
	</owl:Class>
	<owl:Class rdf:about="#OrgEclipseSwtAwtAPI">
		<rdfs:subClassOf rdf:resource="&java;JavaAPI"/>
		<rdfs:comment xml:lang="en">JavaLibrary implementing the org.eclipse.swt.awt package for SWT 3.0</rdfs:comment>
		<rdfs:comment xml:lang="OWLManchester">platform:comprisesInterfacePart some OrgEclipseSwtAwt</rdfs:comment>
	</owl:Class>
	<owl:Class rdf:about="#OrgEclipseSwtBrowserAPI">
		<rdfs:subClassOf rdf:resource="&java;JavaAPI"/>
		<rdfs:comment xml:lang="en">JavaLibrary implementing the org.eclipse.swt.browser package for SWT 3.0</rdfs:comment>
		<rdfs:comment xml:lang="OWLManchester">platform:comprisesInterfacePart some OrgEclipseSwtBrowser</rdfs:comment>
	</owl:Class>
	<owl:Class rdf:about="#OrgEclipseSwtEventsAPI">
		<rdfs:subClassOf rdf:resource="&java;JavaAPI"/>
		<rdfs:comment xml:lang="en">JavaLibrary implementing the org.eclipse.swt.events package for SWT 3.0</rdfs:comment>
		<rdfs:comment xml:lang="OWLManchester">platform:comprisesInterfacePart some OrgEclipseSwtEvents</rdfs:comment>
	</owl:Class>
	<owl:Class rdf:about="#OrgEclipseSwtGraphicsAPI">
		<rdfs:subClassOf rdf:resource="&java;JavaAPI"/>
		<rdfs:comment xml:lang="en">JavaLibrary implementing the org.eclipse.swt.graphics package for SWT 3.0</rdfs:comment>
		<rdfs:comment xml:lang="OWLManchester">platform:comprisesInterfacePart some OrgEclipseSwtGraphics</rdfs:comment>
	</owl:Class>
	<owl:Class rdf:about="#OrgEclipseSwtCustomAPI">
		<rdfs:subClassOf rdf:resource="&java;JavaAPI"/>
		<rdfs:comment xml:lang="en">JavaLibrary implementing the org.eclipse.swt.custom package for SWT 3.0</rdfs:comment>
		<rdfs:comment xml:lang="OWLManchester">platform:comprisesInterfacePart some OrgEclipseSwtCustom</rdfs:comment>
	</owl:Class>
	<owl:Class rdf:about="#OrgEclipseSwtPrintingAPI">
		<rdfs:subClassOf rdf:resource="&java;JavaAPI"/>
		<rdfs:comment xml:lang="en">JavaLibrary implementing the org.eclipse.swt.printing package for SWT 3.0</rdfs:comment>
		<rdfs:comment xml:lang="OWLManchester">platform:comprisesInterfacePart some OrgEclipseSwtPrinting</rdfs:comment>
	</owl:Class>
	<owl:Class rdf:about="#OrgEclipseSwtDndAPI">
		<rdfs:subClassOf rdf:resource="&java;JavaAPI"/>
		<rdfs:comment xml:lang="en">JavaLibrary implementing the org.eclipse.swt.dnd package for SWT 3.0</rdfs:comment>
		<rdfs:comment xml:lang="OWLManchester">platform:comprisesInterfacePart some OrgEclipseSwtDnd</rdfs:comment>
	</owl:Class>
	<owl:Class rdf:about="#OrgEclipseSwtLayoutAPI">
		<rdfs:subClassOf rdf:resource="&java;JavaAPI"/>
		<rdfs:comment xml:lang="en">JavaLibrary implementing the org.eclipse.swt.layout package for SWT 3.0</rdfs:comment>
		<rdfs:comment xml:lang="OWLManchester">platform:comprisesInterfacePart some OrgEclipseSwtLayout</rdfs:comment>
	</owl:Class>
	<owl:Class rdf:about="#OrgEclipseSwtProgramAPI">
		<rdfs:subClassOf rdf:resource="&java;JavaAPI"/>
		<rdfs:comment xml:lang="en">JavaLibrary implementing the org.eclipse.swt.program package for SWT 3.0</rdfs:comment>
		<rdfs:comment xml:lang="OWLManchester">platform:comprisesInterfacePart some OrgEclipseSwtProgram</rdfs:comment>
	</owl:Class>
	<OrgEclipseSwt rdf:about="#theOrgEclipseSwtPart">
	</OrgEclipseSwt>
	<OrgEclipseSwtAccessibility rdf:about="#theOrgEclipseSwtAccessibilityPart">
	</OrgEclipseSwtAccessibility>
	<OrgEclipseSwtWidgets rdf:about="#theOrgEclipseSwtWidgetsPart">
	</OrgEclipseSwtWidgets>
	<OrgEclipseSwtAwt rdf:about="#theOrgEclipseSwtAwtPart">
	</OrgEclipseSwtAwt>
	<OrgEclipseSwtBrowser rdf:about="#theOrgEclipseSwtBrowserPart">
	</OrgEclipseSwtBrowser>
	<OrgEclipseSwtEvents rdf:about="#theOrgEclipseSwtEventsPart">
	</OrgEclipseSwtEvents>
	<OrgEclipseSwtGraphics rdf:about="#theOrgEclipseSwtGraphicsPart">
	</OrgEclipseSwtGraphics>
	<OrgEclipseSwtCustom rdf:about="#theOrgEclipseSwtCustomPart">
	</OrgEclipseSwtCustom>
	<OrgEclipseSwtPrinting rdf:about="#theOrgEclipseSwtPrintingPart">
	</OrgEclipseSwtPrinting>
	<OrgEclipseSwtDnd rdf:about="#theOrgEclipseSwtDndPart">
	</OrgEclipseSwtDnd>
	<OrgEclipseSwtLayout rdf:about="#theOrgEclipseSwtLayoutPart">
	</OrgEclipseSwtLayout>
	<OrgEclipseSwtProgram rdf:about="#theOrgEclipseSwtProgramPart">
	</OrgEclipseSwtProgram>
	<owl:Class rdf:about="#OrgEclipseSwtClassLibrary">
		<rdfs:subClassOf rdf:resource="&java;JavaClassLibrary"/>
		<rdfs:comment xml:lang="en">JavaLibrary implementing the org.eclipse.swt package for SWT 3.0</rdfs:comment>
		<rdfs:comment xml:lang="OWLManchester">platform:implementsInterface some OrgEclipseSwtAPI</rdfs:comment>
	</owl:Class>
	<owl:Class rdf:about="#OrgEclipseSwtAccessibilityClassLibrary">
		<rdfs:subClassOf rdf:resource="&java;JavaClassLibrary"/>
		<rdfs:comment xml:lang="en">JavaLibrary implementing the org.eclipse.swt.accessibility package for SWT 3.0</rdfs:comment>
		<rdfs:comment xml:lang="OWLManchester">platform:implementsInterface some OrgEclipseSwtAccessibilityAPI</rdfs:comment>
	</owl:Class>
	<owl:Class rdf:about="#OrgEclipseSwtWidgetsClassLibrary">
		<rdfs:subClassOf rdf:resource="&java;JavaClassLibrary"/>
		<rdfs:comment xml:lang="en">JavaLibrary implementing the org.eclipse.swt.widgets package for SWT 3.0</rdfs:comment>
		<rdfs:comment xml:lang="OWLManchester">platform:implementsInterface some OrgEclipseSwtWidgetsAPI</rdfs:comment>
	</owl:Class>
	<owl:Class rdf:about="#OrgEclipseSwtAwtClassLibrary">
		<rdfs:subClassOf rdf:resource="&java;JavaClassLibrary"/>
		<rdfs:comment xml:lang="en">JavaLibrary implementing the org.eclipse.swt.awt package for SWT 3.0</rdfs:comment>
		<rdfs:comment xml:lang="OWLManchester">platform:implementsInterface some OrgEclipseSwtAwtAPI</rdfs:comment>
	</owl:Class>
	<owl:Class rdf:about="#OrgEclipseSwtBrowserClassLibrary">
		<rdfs:subClassOf rdf:resource="&java;JavaClassLibrary"/>
		<rdfs:comment xml:lang="en">JavaLibrary implementing the org.eclipse.swt.browser package for SWT 3.0</rdfs:comment>
		<rdfs:comment xml:lang="OWLManchester">platform:implementsInterface some OrgEclipseSwtBrowserAPI</rdfs:comment>
	</owl:Class>
	<owl:Class rdf:about="#OrgEclipseSwtEventsClassLibrary">
		<rdfs:subClassOf rdf:resource="&java;JavaClassLibrary"/>
		<rdfs:comment xml:lang="en">JavaLibrary implementing the org.eclipse.swt.events package for SWT 3.0</rdfs:comment>
		<rdfs:comment xml:lang="OWLManchester">platform:implementsInterface some OrgEclipseSwtEventsAPI</rdfs:comment>
	</owl:Class>
	<owl:Class rdf:about="#OrgEclipseSwtGraphicsClassLibrary">
		<rdfs:subClassOf rdf:resource="&java;JavaClassLibrary"/>
		<rdfs:comment xml:lang="en">JavaLibrary implementing the org.eclipse.swt.graphics package for SWT 3.0</rdfs:comment>
		<rdfs:comment xml:lang="OWLManchester">platform:implementsInterface some OrgEclipseSwtGraphicsAPI</rdfs:comment>
	</owl:Class>
	<owl:Class rdf:about="#OrgEclipseSwtCustomClassLibrary">
		<rdfs:subClassOf rdf:resource="&java;JavaClassLibrary"/>
		<rdfs:comment xml:lang="en">JavaLibrary implementing the org.eclipse.swt.custom package for SWT 3.0</rdfs:comment>
		<rdfs:comment xml:lang="OWLManchester">platform:implementsInterface some OrgEclipseSwtCustomAPI</rdfs:comment>
	</owl:Class>
	<owl:Class rdf:about="#OrgEclipseSwtPrintingClassLibrary">
		<rdfs:subClassOf rdf:resource="&java;JavaClassLibrary"/>
		<rdfs:comment xml:lang="en">JavaLibrary implementing the org.eclipse.swt.printing package for SWT 3.0</rdfs:comment>
		<rdfs:comment xml:lang="OWLManchester">platform:implementsInterface some OrgEclipseSwtPrintingAPI</rdfs:comment>
	</owl:Class>
	<owl:Class rdf:about="#OrgEclipseSwtDndClassLibrary">
		<rdfs:subClassOf rdf:resource="&java;JavaClassLibrary"/>
		<rdfs:comment xml:lang="en">JavaLibrary implementing the org.eclipse.swt.dnd package for SWT 3.0</rdfs:comment>
		<rdfs:comment xml:lang="OWLManchester">platform:implementsInterface some OrgEclipseSwtDndAPI</rdfs:comment>
	</owl:Class>
	<owl:Class rdf:about="#OrgEclipseSwtLayoutClassLibrary">
		<rdfs:subClassOf rdf:resource="&java;JavaClassLibrary"/>
		<rdfs:comment xml:lang="en">JavaLibrary implementing the org.eclipse.swt.layout package for SWT 3.0</rdfs:comment>
		<rdfs:comment xml:lang="OWLManchester">platform:implementsInterface some OrgEclipseSwtLayoutAPI</rdfs:comment>
	</owl:Class>
	<owl:Class rdf:about="#OrgEclipseSwtProgramClassLibrary">
		<rdfs:subClassOf rdf:resource="&java;JavaClassLibrary"/>
		<rdfs:comment xml:lang="en">JavaLibrary implementing the org.eclipse.swt.program package for SWT 3.0</rdfs:comment>
		<rdfs:comment xml:lang="OWLManchester">platform:implementsInterface some OrgEclipseSwtProgramAPI</rdfs:comment>
	</owl:Class>
</rdf:RDF>
