<?xml version="1.0" encoding="ISO-8859-1"?>
<!DOCTYPE rdf:RDF [
	<!ENTITY ns_117 "http://localhost/~dennis/platformkit/2010_1/">
	<!ENTITY swt-3_3 "http://soft.vub.ac.be/platformkit/2010/1/swt-3_3.owl#">
	<!ENTITY platform "http://localhost/~dennis/platformkit/2010_1/platform.owl#">
	<!ENTITY java "http://localhost/~dennis/platformkit/2010_1/java.owl#">
	<!ENTITY swt-3_4 "http://soft.vub.ac.be/platformkit/2010/1/swt-3_4.owl#">
	<!ENTITY xsd "http://www.w3.org/2001/XMLSchema#">
	<!ENTITY isa "http://localhost/~dennis/platformkit/2010_1/isa.owl#">
	<!ENTITY owl "http://www.w3.org/2002/07/owl#">
	<!ENTITY rdf "http://www.w3.org/1999/02/22-rdf-syntax-ns#">
	<!ENTITY rdfs "http://www.w3.org/2000/01/rdf-schema#">
]>
<rdf:RDF
	 xmlns:ns_117="&ns_117;"
	 xmlns:swt-3_3="&swt-3_3;"
	 xmlns:platform="&platform;"
	 xmlns:java="&java;"
	 xmlns:swt-3_4="&swt-3_4;"
	 xmlns:xsd="&xsd;"
	 xmlns:isa="&isa;"
	 xmlns:owl="&owl;"
	 xmlns:rdf="&rdf;"
	 xmlns:rdfs="&rdfs;"
>

	<owl:Ontology rdf:about="http://soft.vub.ac.be/platformkit/2010/1/swt-3_4.owl#">
		<owl:imports rdf:resource="http://localhost/~dennis/platformkit/2010_1/platform.owl"/>
		<owl:imports rdf:resource="http://localhost/~dennis/platformkit/2010_1/java.owl"/>
		<owl:imports rdf:resource="http://soft.vub.ac.be/platformkit/2010/1/swt-3_3.owl#"/>
		<owl:imports rdf:resource="http://localhost/~dennis/platformkit/2010_1/isa.owl"/>
		<rdfs:comment xml:lang="en">Generated by $Id: UML2ToPackageAPIOntology.atl 8068 2010-03-15 10:37:32Z dwagelaa $ and $Id: UML2ToAPIOntology.atl 8068 2010-03-15 10:37:32Z dwagelaa $ and $Id:UML2Comparison.atl 7084 2007-07-10 13:19:05Z dwagelaa $</rdfs:comment>
		<rdfs:label xml:lang="en">SWT 3.4</rdfs:label>
	</owl:Ontology>
	<owl:Class rdf:about="&swt-3_4;SWT3_4API">
		<owl:equivalentClass>
			<owl:Class >
				<owl:intersectionOf rdf:parseType="Collection">
					<owl:Restriction>
						<owl:onProperty rdf:resource="&platform;comprisesInterfacePart"/>
						<owl:someValuesFrom rdf:resource="&swt-3_4;OrgEclipseSwt"/>
					</owl:Restriction>
					<owl:Restriction>
						<owl:onProperty rdf:resource="&platform;comprisesInterfacePart"/>
						<owl:someValuesFrom rdf:resource="&swt-3_4;OrgEclipseSwtAccessibility"/>
					</owl:Restriction>
					<owl:Restriction>
						<owl:onProperty rdf:resource="&platform;comprisesInterfacePart"/>
						<owl:someValuesFrom rdf:resource="&swt-3_4;OrgEclipseSwtWidgets"/>
					</owl:Restriction>
					<owl:Restriction>
						<owl:onProperty rdf:resource="&platform;comprisesInterfacePart"/>
						<owl:someValuesFrom rdf:resource="&swt-3_4;OrgEclipseSwtAwt"/>
					</owl:Restriction>
					<owl:Restriction>
						<owl:onProperty rdf:resource="&platform;comprisesInterfacePart"/>
						<owl:someValuesFrom rdf:resource="&swt-3_4;OrgEclipseSwtBrowser"/>
					</owl:Restriction>
					<owl:Restriction>
						<owl:onProperty rdf:resource="&platform;comprisesInterfacePart"/>
						<owl:someValuesFrom rdf:resource="&swt-3_4;OrgEclipseSwtEvents"/>
					</owl:Restriction>
					<owl:Restriction>
						<owl:onProperty rdf:resource="&platform;comprisesInterfacePart"/>
						<owl:someValuesFrom rdf:resource="&swt-3_4;OrgEclipseSwtGraphics"/>
					</owl:Restriction>
					<owl:Restriction>
						<owl:onProperty rdf:resource="&platform;comprisesInterfacePart"/>
						<owl:someValuesFrom rdf:resource="&swt-3_4;OrgEclipseSwtCustom"/>
					</owl:Restriction>
					<owl:Restriction>
						<owl:onProperty rdf:resource="&platform;comprisesInterfacePart"/>
						<owl:someValuesFrom rdf:resource="&swt-3_4;OrgEclipseSwtPrinting"/>
					</owl:Restriction>
					<owl:Restriction>
						<owl:onProperty rdf:resource="&platform;comprisesInterfacePart"/>
						<owl:someValuesFrom rdf:resource="&swt-3_4;OrgEclipseSwtDnd"/>
					</owl:Restriction>
					<owl:Restriction>
						<owl:onProperty rdf:resource="&platform;comprisesInterfacePart"/>
						<owl:someValuesFrom rdf:resource="&swt-3_4;OrgEclipseSwtLayout"/>
					</owl:Restriction>
					<owl:Restriction>
						<owl:onProperty rdf:resource="&platform;comprisesInterfacePart"/>
						<owl:someValuesFrom rdf:resource="&swt-3_4;OrgEclipseSwtOpengl"/>
					</owl:Restriction>
					<owl:Restriction>
						<owl:onProperty rdf:resource="&platform;comprisesInterfacePart"/>
						<owl:someValuesFrom rdf:resource="&swt-3_4;OrgEclipseSwtProgram"/>
					</owl:Restriction>
				</owl:intersectionOf>
			</owl:Class>
		</owl:equivalentClass>
		<rdfs:subClassOf rdf:resource="&java;JavaAPI"/>
		<rdfs:comment xml:lang="en">SWT 3.4 API</rdfs:comment>
	</owl:Class>
	<swt-3_4:SWT3_4API rdf:about="&swt-3_4;theSWT3_4API">
		<platform:comprisesInterfacePart rdf:resource="&swt-3_4;theOrgEclipseSwtProgramPart"/>
		<platform:comprisesInterfacePart rdf:resource="&swt-3_4;theOrgEclipseSwtOpenglPart"/>
		<platform:comprisesInterfacePart rdf:resource="&swt-3_4;theOrgEclipseSwtLayoutPart"/>
		<platform:comprisesInterfacePart rdf:resource="&swt-3_4;theOrgEclipseSwtDndPart"/>
		<platform:comprisesInterfacePart rdf:resource="&swt-3_4;theOrgEclipseSwtPrintingPart"/>
		<platform:comprisesInterfacePart rdf:resource="&swt-3_4;theOrgEclipseSwtCustomPart"/>
		<platform:comprisesInterfacePart rdf:resource="&swt-3_4;theOrgEclipseSwtGraphicsPart"/>
		<platform:comprisesInterfacePart rdf:resource="&swt-3_4;theOrgEclipseSwtEventsPart"/>
		<platform:comprisesInterfacePart rdf:resource="&swt-3_4;theOrgEclipseSwtBrowserPart"/>
		<platform:comprisesInterfacePart rdf:resource="&swt-3_4;theOrgEclipseSwtAwtPart"/>
		<platform:comprisesInterfacePart rdf:resource="&swt-3_4;theOrgEclipseSwtWidgetsPart"/>
		<platform:comprisesInterfacePart rdf:resource="&swt-3_4;theOrgEclipseSwtAccessibilityPart"/>
		<platform:comprisesInterfacePart rdf:resource="&swt-3_4;theOrgEclipseSwtPart"/>
	</swt-3_4:SWT3_4API>
	<owl:Class rdf:about="&swt-3_4;SWT3_4ClassLibrary">
		<owl:equivalentClass>
			<owl:Restriction>
				<owl:onProperty rdf:resource="&platform;implementsInterface"/>
				<owl:someValuesFrom rdf:resource="&swt-3_4;SWT3_4API"/>
			</owl:Restriction>
		</owl:equivalentClass>
		<rdfs:subClassOf rdf:resource="&java;JavaClassLibrary"/>
		<rdfs:comment xml:lang="en">Java class library implementing the SWT 3.4 API</rdfs:comment>
	</owl:Class>
	<owl:Class rdf:about="&swt-3_4;SWT3_4BytecodeFormat">
		<rdfs:subClassOf rdf:resource="&isa;JavaBytecode"/>
		<rdfs:comment xml:lang="en">SWT 3.4 bytecode format</rdfs:comment>
	</owl:Class>
	<swt-3_4:SWT3_4BytecodeFormat rdf:about="&swt-3_4;theSWT3_4BytecodeFormat">
	</swt-3_4:SWT3_4BytecodeFormat>
	<owl:Class rdf:about="&swt-3_4;SWT3_4VM">
		<owl:equivalentClass>
			<owl:Restriction>
				<owl:onProperty rdf:resource="&platform;implementsInterface"/>
				<owl:someValuesFrom rdf:resource="&swt-3_4;SWT3_4BytecodeFormat"/>
			</owl:Restriction>
		</owl:equivalentClass>
		<rdfs:subClassOf rdf:resource="&java;JavaVM"/>
		<rdfs:comment xml:lang="en">SWT 3.4 virtual machine</rdfs:comment>
	</owl:Class>
	<owl:Class rdf:about="&swt-3_4;SWT3_4JRE">
		<owl:equivalentClass>
			<owl:Class >
				<owl:intersectionOf rdf:parseType="Collection">
					<owl:Restriction>
						<owl:onProperty rdf:resource="&platform;providesFeature"/>
						<owl:someValuesFrom rdf:resource="&swt-3_4;SWT3_4ClassLibrary"/>
					</owl:Restriction>
					<owl:Restriction>
						<owl:onProperty rdf:resource="&platform;providesFeature"/>
						<owl:someValuesFrom rdf:resource="&swt-3_4;SWT3_4VM"/>
					</owl:Restriction>
				</owl:intersectionOf>
			</owl:Class>
		</owl:equivalentClass>
		<rdfs:subClassOf rdf:resource="&java;JRE"/>
		<rdfs:comment xml:lang="en">SWT 3.4 Java Runtime Environment</rdfs:comment>
	</owl:Class>
	<owl:Class rdf:about="&swt-3_4;OrgEclipseSwt">
		<rdfs:subClassOf rdf:resource="&swt-3_3;OrgEclipseSwt"/>
		<rdfs:comment xml:lang="en">Java API part implementing the org.eclipse.swt package for SWT 3.4</rdfs:comment>
	</owl:Class>
	<owl:Class rdf:about="&swt-3_4;OrgEclipseSwtAccessibility">
		<owl:equivalentClass rdf:resource="&swt-3_3;OrgEclipseSwtAccessibility"/>
		<rdfs:subClassOf rdf:resource="&java;JavaAPIPart"/>
		<rdfs:seeAlso rdf:resource="&swt-3_4;OrgEclipseSwtWidgets"/>
		<rdfs:comment xml:lang="en">Java API part implementing the org.eclipse.swt.accessibility package for SWT 3.4</rdfs:comment>
	</owl:Class>
	<owl:Class rdf:about="&swt-3_4;OrgEclipseSwtWidgets">
		<rdfs:subClassOf rdf:resource="&swt-3_3;OrgEclipseSwtWidgets"/>
		<rdfs:seeAlso rdf:resource="&swt-3_4;OrgEclipseSwtGraphics"/>
		<rdfs:seeAlso rdf:resource="&swt-3_4;OrgEclipseSwtEvents"/>
		<rdfs:seeAlso rdf:resource="&swt-3_4;OrgEclipseSwtAccessibility"/>
		<rdfs:comment xml:lang="en">Java API part implementing the org.eclipse.swt.widgets package for SWT 3.4</rdfs:comment>
	</owl:Class>
	<owl:Class rdf:about="&swt-3_4;OrgEclipseSwtAwt">
		<owl:equivalentClass rdf:resource="&swt-3_3;OrgEclipseSwtAwt"/>
		<rdfs:subClassOf rdf:resource="&java;JavaAPIPart"/>
		<rdfs:seeAlso rdf:resource="&swt-3_4;OrgEclipseSwtWidgets"/>
		<rdfs:comment xml:lang="en">Java API part implementing the org.eclipse.swt.awt package for SWT 3.4</rdfs:comment>
	</owl:Class>
	<owl:Class rdf:about="&swt-3_4;OrgEclipseSwtBrowser">
		<rdfs:subClassOf rdf:resource="&swt-3_3;OrgEclipseSwtBrowser"/>
		<rdfs:seeAlso rdf:resource="&swt-3_4;OrgEclipseSwtEvents"/>
		<rdfs:seeAlso rdf:resource="&swt-3_4;OrgEclipseSwtWidgets"/>
		<rdfs:seeAlso rdf:resource="&swt-3_4;OrgEclipseSwtGraphics"/>
		<rdfs:comment xml:lang="en">Java API part implementing the org.eclipse.swt.browser package for SWT 3.4</rdfs:comment>
	</owl:Class>
	<owl:Class rdf:about="&swt-3_4;OrgEclipseSwtEvents">
		<owl:equivalentClass rdf:resource="&swt-3_3;OrgEclipseSwtEvents"/>
		<rdfs:subClassOf rdf:resource="&java;JavaAPIPart"/>
		<rdfs:seeAlso rdf:resource="&swt-3_4;OrgEclipseSwtWidgets"/>
		<rdfs:seeAlso rdf:resource="&swt-3_4;OrgEclipseSwtGraphics"/>
		<rdfs:comment xml:lang="en">Java API part implementing the org.eclipse.swt.events package for SWT 3.4</rdfs:comment>
	</owl:Class>
	<owl:Class rdf:about="&swt-3_4;OrgEclipseSwtGraphics">
		<rdfs:subClassOf rdf:resource="&swt-3_3;OrgEclipseSwtGraphics"/>
		<rdfs:comment xml:lang="en">Java API part implementing the org.eclipse.swt.graphics package for SWT 3.4</rdfs:comment>
	</owl:Class>
	<owl:Class rdf:about="&swt-3_4;OrgEclipseSwtCustom">
		<rdfs:subClassOf rdf:resource="&swt-3_3;OrgEclipseSwtCustom"/>
		<rdfs:seeAlso rdf:resource="&swt-3_4;OrgEclipseSwtGraphics"/>
		<rdfs:seeAlso rdf:resource="&swt-3_4;OrgEclipseSwtEvents"/>
		<rdfs:seeAlso rdf:resource="&swt-3_4;OrgEclipseSwtPrinting"/>
		<rdfs:seeAlso rdf:resource="&swt-3_4;OrgEclipseSwtWidgets"/>
		<rdfs:seeAlso rdf:resource="&swt-3_4;OrgEclipseSwtDnd"/>
		<rdfs:comment xml:lang="en">Java API part implementing the org.eclipse.swt.custom package for SWT 3.4</rdfs:comment>
	</owl:Class>
	<owl:Class rdf:about="&swt-3_4;OrgEclipseSwtPrinting">
		<rdfs:subClassOf rdf:resource="&swt-3_3;OrgEclipseSwtPrinting"/>
		<rdfs:seeAlso rdf:resource="&swt-3_4;OrgEclipseSwtWidgets"/>
		<rdfs:seeAlso rdf:resource="&swt-3_4;OrgEclipseSwtGraphics"/>
		<rdfs:comment xml:lang="en">Java API part implementing the org.eclipse.swt.printing package for SWT 3.4</rdfs:comment>
	</owl:Class>
	<owl:Class rdf:about="&swt-3_4;OrgEclipseSwtDnd">
		<rdfs:subClassOf rdf:resource="&swt-3_3;OrgEclipseSwtDnd"/>
		<rdfs:seeAlso rdf:resource="&swt-3_4;OrgEclipseSwtEvents"/>
		<rdfs:seeAlso rdf:resource="&swt-3_4;OrgEclipseSwtWidgets"/>
		<rdfs:seeAlso rdf:resource="&swt-3_4;OrgEclipseSwtGraphics"/>
		<rdfs:comment xml:lang="en">Java API part implementing the org.eclipse.swt.dnd package for SWT 3.4</rdfs:comment>
	</owl:Class>
	<owl:Class rdf:about="&swt-3_4;OrgEclipseSwtLayout">
		<rdfs:subClassOf rdf:resource="&swt-3_3;OrgEclipseSwtLayout"/>
		<rdfs:seeAlso rdf:resource="&swt-3_4;OrgEclipseSwtWidgets"/>
		<rdfs:seeAlso rdf:resource="&swt-3_4;OrgEclipseSwtGraphics"/>
		<rdfs:comment xml:lang="en">Java API part implementing the org.eclipse.swt.layout package for SWT 3.4</rdfs:comment>
	</owl:Class>
	<owl:Class rdf:about="&swt-3_4;OrgEclipseSwtOpengl">
		<rdfs:subClassOf rdf:resource="&swt-3_3;OrgEclipseSwtOpengl"/>
		<rdfs:seeAlso rdf:resource="&swt-3_4;OrgEclipseSwtWidgets"/>
		<rdfs:comment xml:lang="en">Java API part implementing the org.eclipse.swt.opengl package for SWT 3.4</rdfs:comment>
	</owl:Class>
	<owl:Class rdf:about="&swt-3_4;OrgEclipseSwtProgram">
		<owl:equivalentClass rdf:resource="&swt-3_3;OrgEclipseSwtProgram"/>
		<rdfs:subClassOf rdf:resource="&java;JavaAPIPart"/>
		<rdfs:seeAlso rdf:resource="&swt-3_4;OrgEclipseSwtGraphics"/>
		<rdfs:comment xml:lang="en">Java API part implementing the org.eclipse.swt.program package for SWT 3.4</rdfs:comment>
	</owl:Class>
	<owl:Class rdf:about="&swt-3_4;OrgEclipseSwtAPI">
		<owl:equivalentClass>
			<owl:Restriction>
				<owl:onProperty rdf:resource="&platform;comprisesInterfacePart"/>
				<owl:someValuesFrom rdf:resource="&swt-3_4;OrgEclipseSwt"/>
			</owl:Restriction>
		</owl:equivalentClass>
		<rdfs:subClassOf rdf:resource="&java;JavaAPI"/>
		<rdfs:comment xml:lang="en">JavaLibrary implementing the org.eclipse.swt package for SWT 3.4</rdfs:comment>
	</owl:Class>
	<owl:Class rdf:about="&swt-3_4;OrgEclipseSwtAccessibilityAPI">
		<owl:equivalentClass>
			<owl:Restriction>
				<owl:onProperty rdf:resource="&platform;comprisesInterfacePart"/>
				<owl:someValuesFrom rdf:resource="&swt-3_4;OrgEclipseSwtAccessibility"/>
			</owl:Restriction>
		</owl:equivalentClass>
		<rdfs:subClassOf rdf:resource="&java;JavaAPI"/>
		<rdfs:comment xml:lang="en">JavaLibrary implementing the org.eclipse.swt.accessibility package for SWT 3.4</rdfs:comment>
	</owl:Class>
	<owl:Class rdf:about="&swt-3_4;OrgEclipseSwtWidgetsAPI">
		<owl:equivalentClass>
			<owl:Restriction>
				<owl:onProperty rdf:resource="&platform;comprisesInterfacePart"/>
				<owl:someValuesFrom rdf:resource="&swt-3_4;OrgEclipseSwtWidgets"/>
			</owl:Restriction>
		</owl:equivalentClass>
		<rdfs:subClassOf rdf:resource="&java;JavaAPI"/>
		<rdfs:comment xml:lang="en">JavaLibrary implementing the org.eclipse.swt.widgets package for SWT 3.4</rdfs:comment>
	</owl:Class>
	<owl:Class rdf:about="&swt-3_4;OrgEclipseSwtAwtAPI">
		<owl:equivalentClass>
			<owl:Restriction>
				<owl:onProperty rdf:resource="&platform;comprisesInterfacePart"/>
				<owl:someValuesFrom rdf:resource="&swt-3_4;OrgEclipseSwtAwt"/>
			</owl:Restriction>
		</owl:equivalentClass>
		<rdfs:subClassOf rdf:resource="&java;JavaAPI"/>
		<rdfs:comment xml:lang="en">JavaLibrary implementing the org.eclipse.swt.awt package for SWT 3.4</rdfs:comment>
	</owl:Class>
	<owl:Class rdf:about="&swt-3_4;OrgEclipseSwtBrowserAPI">
		<owl:equivalentClass>
			<owl:Restriction>
				<owl:onProperty rdf:resource="&platform;comprisesInterfacePart"/>
				<owl:someValuesFrom rdf:resource="&swt-3_4;OrgEclipseSwtBrowser"/>
			</owl:Restriction>
		</owl:equivalentClass>
		<rdfs:subClassOf rdf:resource="&java;JavaAPI"/>
		<rdfs:comment xml:lang="en">JavaLibrary implementing the org.eclipse.swt.browser package for SWT 3.4</rdfs:comment>
	</owl:Class>
	<owl:Class rdf:about="&swt-3_4;OrgEclipseSwtEventsAPI">
		<owl:equivalentClass>
			<owl:Restriction>
				<owl:onProperty rdf:resource="&platform;comprisesInterfacePart"/>
				<owl:someValuesFrom rdf:resource="&swt-3_4;OrgEclipseSwtEvents"/>
			</owl:Restriction>
		</owl:equivalentClass>
		<rdfs:subClassOf rdf:resource="&java;JavaAPI"/>
		<rdfs:comment xml:lang="en">JavaLibrary implementing the org.eclipse.swt.events package for SWT 3.4</rdfs:comment>
	</owl:Class>
	<owl:Class rdf:about="&swt-3_4;OrgEclipseSwtGraphicsAPI">
		<owl:equivalentClass>
			<owl:Restriction>
				<owl:onProperty rdf:resource="&platform;comprisesInterfacePart"/>
				<owl:someValuesFrom rdf:resource="&swt-3_4;OrgEclipseSwtGraphics"/>
			</owl:Restriction>
		</owl:equivalentClass>
		<rdfs:subClassOf rdf:resource="&java;JavaAPI"/>
		<rdfs:comment xml:lang="en">JavaLibrary implementing the org.eclipse.swt.graphics package for SWT 3.4</rdfs:comment>
	</owl:Class>
	<owl:Class rdf:about="&swt-3_4;OrgEclipseSwtCustomAPI">
		<owl:equivalentClass>
			<owl:Restriction>
				<owl:onProperty rdf:resource="&platform;comprisesInterfacePart"/>
				<owl:someValuesFrom rdf:resource="&swt-3_4;OrgEclipseSwtCustom"/>
			</owl:Restriction>
		</owl:equivalentClass>
		<rdfs:subClassOf rdf:resource="&java;JavaAPI"/>
		<rdfs:comment xml:lang="en">JavaLibrary implementing the org.eclipse.swt.custom package for SWT 3.4</rdfs:comment>
	</owl:Class>
	<owl:Class rdf:about="&swt-3_4;OrgEclipseSwtPrintingAPI">
		<owl:equivalentClass>
			<owl:Restriction>
				<owl:onProperty rdf:resource="&platform;comprisesInterfacePart"/>
				<owl:someValuesFrom rdf:resource="&swt-3_4;OrgEclipseSwtPrinting"/>
			</owl:Restriction>
		</owl:equivalentClass>
		<rdfs:subClassOf rdf:resource="&java;JavaAPI"/>
		<rdfs:comment xml:lang="en">JavaLibrary implementing the org.eclipse.swt.printing package for SWT 3.4</rdfs:comment>
	</owl:Class>
	<owl:Class rdf:about="&swt-3_4;OrgEclipseSwtDndAPI">
		<owl:equivalentClass>
			<owl:Restriction>
				<owl:onProperty rdf:resource="&platform;comprisesInterfacePart"/>
				<owl:someValuesFrom rdf:resource="&swt-3_4;OrgEclipseSwtDnd"/>
			</owl:Restriction>
		</owl:equivalentClass>
		<rdfs:subClassOf rdf:resource="&java;JavaAPI"/>
		<rdfs:comment xml:lang="en">JavaLibrary implementing the org.eclipse.swt.dnd package for SWT 3.4</rdfs:comment>
	</owl:Class>
	<owl:Class rdf:about="&swt-3_4;OrgEclipseSwtLayoutAPI">
		<owl:equivalentClass>
			<owl:Restriction>
				<owl:onProperty rdf:resource="&platform;comprisesInterfacePart"/>
				<owl:someValuesFrom rdf:resource="&swt-3_4;OrgEclipseSwtLayout"/>
			</owl:Restriction>
		</owl:equivalentClass>
		<rdfs:subClassOf rdf:resource="&java;JavaAPI"/>
		<rdfs:comment xml:lang="en">JavaLibrary implementing the org.eclipse.swt.layout package for SWT 3.4</rdfs:comment>
	</owl:Class>
	<owl:Class rdf:about="&swt-3_4;OrgEclipseSwtOpenglAPI">
		<owl:equivalentClass>
			<owl:Restriction>
				<owl:onProperty rdf:resource="&platform;comprisesInterfacePart"/>
				<owl:someValuesFrom rdf:resource="&swt-3_4;OrgEclipseSwtOpengl"/>
			</owl:Restriction>
		</owl:equivalentClass>
		<rdfs:subClassOf rdf:resource="&java;JavaAPI"/>
		<rdfs:comment xml:lang="en">JavaLibrary implementing the org.eclipse.swt.opengl package for SWT 3.4</rdfs:comment>
	</owl:Class>
	<owl:Class rdf:about="&swt-3_4;OrgEclipseSwtProgramAPI">
		<owl:equivalentClass>
			<owl:Restriction>
				<owl:onProperty rdf:resource="&platform;comprisesInterfacePart"/>
				<owl:someValuesFrom rdf:resource="&swt-3_4;OrgEclipseSwtProgram"/>
			</owl:Restriction>
		</owl:equivalentClass>
		<rdfs:subClassOf rdf:resource="&java;JavaAPI"/>
		<rdfs:comment xml:lang="en">JavaLibrary implementing the org.eclipse.swt.program package for SWT 3.4</rdfs:comment>
	</owl:Class>
	<swt-3_4:OrgEclipseSwt rdf:about="&swt-3_4;theOrgEclipseSwtPart">
	</swt-3_4:OrgEclipseSwt>
	<swt-3_4:OrgEclipseSwtAccessibility rdf:about="&swt-3_4;theOrgEclipseSwtAccessibilityPart">
	</swt-3_4:OrgEclipseSwtAccessibility>
	<swt-3_4:OrgEclipseSwtWidgets rdf:about="&swt-3_4;theOrgEclipseSwtWidgetsPart">
	</swt-3_4:OrgEclipseSwtWidgets>
	<swt-3_4:OrgEclipseSwtAwt rdf:about="&swt-3_4;theOrgEclipseSwtAwtPart">
	</swt-3_4:OrgEclipseSwtAwt>
	<swt-3_4:OrgEclipseSwtBrowser rdf:about="&swt-3_4;theOrgEclipseSwtBrowserPart">
	</swt-3_4:OrgEclipseSwtBrowser>
	<swt-3_4:OrgEclipseSwtEvents rdf:about="&swt-3_4;theOrgEclipseSwtEventsPart">
	</swt-3_4:OrgEclipseSwtEvents>
	<swt-3_4:OrgEclipseSwtGraphics rdf:about="&swt-3_4;theOrgEclipseSwtGraphicsPart">
	</swt-3_4:OrgEclipseSwtGraphics>
	<swt-3_4:OrgEclipseSwtCustom rdf:about="&swt-3_4;theOrgEclipseSwtCustomPart">
	</swt-3_4:OrgEclipseSwtCustom>
	<swt-3_4:OrgEclipseSwtPrinting rdf:about="&swt-3_4;theOrgEclipseSwtPrintingPart">
	</swt-3_4:OrgEclipseSwtPrinting>
	<swt-3_4:OrgEclipseSwtDnd rdf:about="&swt-3_4;theOrgEclipseSwtDndPart">
	</swt-3_4:OrgEclipseSwtDnd>
	<swt-3_4:OrgEclipseSwtLayout rdf:about="&swt-3_4;theOrgEclipseSwtLayoutPart">
	</swt-3_4:OrgEclipseSwtLayout>
	<swt-3_4:OrgEclipseSwtOpengl rdf:about="&swt-3_4;theOrgEclipseSwtOpenglPart">
	</swt-3_4:OrgEclipseSwtOpengl>
	<swt-3_4:OrgEclipseSwtProgram rdf:about="&swt-3_4;theOrgEclipseSwtProgramPart">
	</swt-3_4:OrgEclipseSwtProgram>
	<owl:Class rdf:about="&swt-3_4;OrgEclipseSwtClassLibrary">
		<owl:equivalentClass>
			<owl:Restriction>
				<owl:onProperty rdf:resource="&platform;implementsInterface"/>
				<owl:someValuesFrom rdf:resource="&swt-3_4;OrgEclipseSwtAPI"/>
			</owl:Restriction>
		</owl:equivalentClass>
		<rdfs:subClassOf rdf:resource="&java;JavaClassLibrary"/>
		<rdfs:comment xml:lang="en">JavaLibrary implementing the org.eclipse.swt package for SWT 3.4</rdfs:comment>
	</owl:Class>
	<owl:Class rdf:about="&swt-3_4;OrgEclipseSwtAccessibilityClassLibrary">
		<owl:equivalentClass>
			<owl:Restriction>
				<owl:onProperty rdf:resource="&platform;implementsInterface"/>
				<owl:someValuesFrom rdf:resource="&swt-3_4;OrgEclipseSwtAccessibilityAPI"/>
			</owl:Restriction>
		</owl:equivalentClass>
		<rdfs:subClassOf rdf:resource="&java;JavaClassLibrary"/>
		<rdfs:comment xml:lang="en">JavaLibrary implementing the org.eclipse.swt.accessibility package for SWT 3.4</rdfs:comment>
	</owl:Class>
	<owl:Class rdf:about="&swt-3_4;OrgEclipseSwtWidgetsClassLibrary">
		<owl:equivalentClass>
			<owl:Restriction>
				<owl:onProperty rdf:resource="&platform;implementsInterface"/>
				<owl:someValuesFrom rdf:resource="&swt-3_4;OrgEclipseSwtWidgetsAPI"/>
			</owl:Restriction>
		</owl:equivalentClass>
		<rdfs:subClassOf rdf:resource="&java;JavaClassLibrary"/>
		<rdfs:comment xml:lang="en">JavaLibrary implementing the org.eclipse.swt.widgets package for SWT 3.4</rdfs:comment>
	</owl:Class>
	<owl:Class rdf:about="&swt-3_4;OrgEclipseSwtAwtClassLibrary">
		<owl:equivalentClass>
			<owl:Restriction>
				<owl:onProperty rdf:resource="&platform;implementsInterface"/>
				<owl:someValuesFrom rdf:resource="&swt-3_4;OrgEclipseSwtAwtAPI"/>
			</owl:Restriction>
		</owl:equivalentClass>
		<rdfs:subClassOf rdf:resource="&java;JavaClassLibrary"/>
		<rdfs:comment xml:lang="en">JavaLibrary implementing the org.eclipse.swt.awt package for SWT 3.4</rdfs:comment>
	</owl:Class>
	<owl:Class rdf:about="&swt-3_4;OrgEclipseSwtBrowserClassLibrary">
		<owl:equivalentClass>
			<owl:Restriction>
				<owl:onProperty rdf:resource="&platform;implementsInterface"/>
				<owl:someValuesFrom rdf:resource="&swt-3_4;OrgEclipseSwtBrowserAPI"/>
			</owl:Restriction>
		</owl:equivalentClass>
		<rdfs:subClassOf rdf:resource="&java;JavaClassLibrary"/>
		<rdfs:comment xml:lang="en">JavaLibrary implementing the org.eclipse.swt.browser package for SWT 3.4</rdfs:comment>
	</owl:Class>
	<owl:Class rdf:about="&swt-3_4;OrgEclipseSwtEventsClassLibrary">
		<owl:equivalentClass>
			<owl:Restriction>
				<owl:onProperty rdf:resource="&platform;implementsInterface"/>
				<owl:someValuesFrom rdf:resource="&swt-3_4;OrgEclipseSwtEventsAPI"/>
			</owl:Restriction>
		</owl:equivalentClass>
		<rdfs:subClassOf rdf:resource="&java;JavaClassLibrary"/>
		<rdfs:comment xml:lang="en">JavaLibrary implementing the org.eclipse.swt.events package for SWT 3.4</rdfs:comment>
	</owl:Class>
	<owl:Class rdf:about="&swt-3_4;OrgEclipseSwtGraphicsClassLibrary">
		<owl:equivalentClass>
			<owl:Restriction>
				<owl:onProperty rdf:resource="&platform;implementsInterface"/>
				<owl:someValuesFrom rdf:resource="&swt-3_4;OrgEclipseSwtGraphicsAPI"/>
			</owl:Restriction>
		</owl:equivalentClass>
		<rdfs:subClassOf rdf:resource="&java;JavaClassLibrary"/>
		<rdfs:comment xml:lang="en">JavaLibrary implementing the org.eclipse.swt.graphics package for SWT 3.4</rdfs:comment>
	</owl:Class>
	<owl:Class rdf:about="&swt-3_4;OrgEclipseSwtCustomClassLibrary">
		<owl:equivalentClass>
			<owl:Restriction>
				<owl:onProperty rdf:resource="&platform;implementsInterface"/>
				<owl:someValuesFrom rdf:resource="&swt-3_4;OrgEclipseSwtCustomAPI"/>
			</owl:Restriction>
		</owl:equivalentClass>
		<rdfs:subClassOf rdf:resource="&java;JavaClassLibrary"/>
		<rdfs:comment xml:lang="en">JavaLibrary implementing the org.eclipse.swt.custom package for SWT 3.4</rdfs:comment>
	</owl:Class>
	<owl:Class rdf:about="&swt-3_4;OrgEclipseSwtPrintingClassLibrary">
		<owl:equivalentClass>
			<owl:Restriction>
				<owl:onProperty rdf:resource="&platform;implementsInterface"/>
				<owl:someValuesFrom rdf:resource="&swt-3_4;OrgEclipseSwtPrintingAPI"/>
			</owl:Restriction>
		</owl:equivalentClass>
		<rdfs:subClassOf rdf:resource="&java;JavaClassLibrary"/>
		<rdfs:comment xml:lang="en">JavaLibrary implementing the org.eclipse.swt.printing package for SWT 3.4</rdfs:comment>
	</owl:Class>
	<owl:Class rdf:about="&swt-3_4;OrgEclipseSwtDndClassLibrary">
		<owl:equivalentClass>
			<owl:Restriction>
				<owl:onProperty rdf:resource="&platform;implementsInterface"/>
				<owl:someValuesFrom rdf:resource="&swt-3_4;OrgEclipseSwtDndAPI"/>
			</owl:Restriction>
		</owl:equivalentClass>
		<rdfs:subClassOf rdf:resource="&java;JavaClassLibrary"/>
		<rdfs:comment xml:lang="en">JavaLibrary implementing the org.eclipse.swt.dnd package for SWT 3.4</rdfs:comment>
	</owl:Class>
	<owl:Class rdf:about="&swt-3_4;OrgEclipseSwtLayoutClassLibrary">
		<owl:equivalentClass>
			<owl:Restriction>
				<owl:onProperty rdf:resource="&platform;implementsInterface"/>
				<owl:someValuesFrom rdf:resource="&swt-3_4;OrgEclipseSwtLayoutAPI"/>
			</owl:Restriction>
		</owl:equivalentClass>
		<rdfs:subClassOf rdf:resource="&java;JavaClassLibrary"/>
		<rdfs:comment xml:lang="en">JavaLibrary implementing the org.eclipse.swt.layout package for SWT 3.4</rdfs:comment>
	</owl:Class>
	<owl:Class rdf:about="&swt-3_4;OrgEclipseSwtOpenglClassLibrary">
		<owl:equivalentClass>
			<owl:Restriction>
				<owl:onProperty rdf:resource="&platform;implementsInterface"/>
				<owl:someValuesFrom rdf:resource="&swt-3_4;OrgEclipseSwtOpenglAPI"/>
			</owl:Restriction>
		</owl:equivalentClass>
		<rdfs:subClassOf rdf:resource="&java;JavaClassLibrary"/>
		<rdfs:comment xml:lang="en">JavaLibrary implementing the org.eclipse.swt.opengl package for SWT 3.4</rdfs:comment>
	</owl:Class>
	<owl:Class rdf:about="&swt-3_4;OrgEclipseSwtProgramClassLibrary">
		<owl:equivalentClass>
			<owl:Restriction>
				<owl:onProperty rdf:resource="&platform;implementsInterface"/>
				<owl:someValuesFrom rdf:resource="&swt-3_4;OrgEclipseSwtProgramAPI"/>
			</owl:Restriction>
		</owl:equivalentClass>
		<rdfs:subClassOf rdf:resource="&java;JavaClassLibrary"/>
		<rdfs:comment xml:lang="en">JavaLibrary implementing the org.eclipse.swt.program package for SWT 3.4</rdfs:comment>
	</owl:Class>
</rdf:RDF>
