<?xml version="1.0" encoding="ISO-8859-1"?>
<!DOCTYPE rdf:RDF [
	<!ENTITY xsd "http://www.w3.org/2001/XMLSchema#">
	<!ENTITY j2me-pp-1_0 "http://soft.vub.ac.be/platformkit/2010/1/j2me-pp-1_0.owl#">
	<!ENTITY platform "http://soft.vub.ac.be/platformkit/2010/1/platform.owl#">
	<!ENTITY java "http://soft.vub.ac.be/platformkit/2010/1/java.owl#">
	<!ENTITY j2se-1_3 "http://soft.vub.ac.be/platformkit/2010/1/j2se-1_3.owl#">
	<!ENTITY isa "http://soft.vub.ac.be/platformkit/2010/1/isa.owl#">
	<!ENTITY rdf "http://www.w3.org/1999/02/22-rdf-syntax-ns#">
	<!ENTITY rdfs "http://www.w3.org/2000/01/rdf-schema#">
	<!ENTITY owl "http://www.w3.org/2002/07/owl#">
]>
<rdf:RDF
	 xmlns="http://soft.vub.ac.be/platformkit/2010/1/j2me-pp-1_1.owl#"
	 xml:base="http://soft.vub.ac.be/platformkit/2010/1/j2me-pp-1_1.owl"
	 xmlns:xsd="&xsd;"
	 xmlns:j2me-pp-1_0="&j2me-pp-1_0;"
	 xmlns:platform="&platform;"
	 xmlns:java="&java;"
	 xmlns:j2se-1_3="&j2se-1_3;"
	 xmlns:isa="&isa;"
	 xmlns:rdf="&rdf;"
	 xmlns:rdfs="&rdfs;"
	 xmlns:owl="&owl;"
>

	<owl:Ontology rdf:about="">
		<owl:versionInfo>$Id$</owl:versionInfo>
		<owl:imports rdf:resource="http://soft.vub.ac.be/platformkit/2010/1/platform.owl"/>
		<owl:imports rdf:resource="http://soft.vub.ac.be/platformkit/2010/1/java.owl"/>
		<owl:imports rdf:resource="http://soft.vub.ac.be/platformkit/2010/1/j2se-1_3.owl"/>
		<owl:imports rdf:resource="http://soft.vub.ac.be/platformkit/2010/1/isa.owl"/>
		<owl:imports rdf:resource="http://soft.vub.ac.be/platformkit/2010/1/j2me-pp-1_0.owl"/>
		<rdfs:comment xml:lang="en">Generated by [UML2ToSimplifiedPackageAPIOntology.atl 8080 2010-03-18 10:46:40Z dwagelaa], [UML2ToPackageAPIOntology.atl 8082 2010-03-18 21:11:00Z dwagelaa], [UML2ToAPIOntology.atl 8082 2010-03-18 21:11:00Z dwagelaa], and [UML2Comparison.atl 8082 2010-03-18 21:11:00Z dwagelaa]</rdfs:comment>
		<rdfs:comment>Dennis Wagelaar &lt;dennis.wagelaar@vub.ac.be&gt;</rdfs:comment>
		<rdfs:comment xml:lang="en">&#169; 2010, Vrije Universiteit Brussel. All rights reserved.</rdfs:comment>
		<rdfs:label xml:lang="en">J2ME PP 1.1</rdfs:label>
	</owl:Ontology>
	<owl:Class rdf:about="#J2MEPP1_1API">
		<rdfs:subClassOf rdf:resource="#JavaIoAPI"/>
		<rdfs:subClassOf rdf:resource="#JavaLangAPI"/>
		<rdfs:subClassOf rdf:resource="#JavaLangRefAPI"/>
		<rdfs:subClassOf rdf:resource="#JavaLangReflectAPI"/>
		<rdfs:subClassOf rdf:resource="#JavaSecurityAPI"/>
		<rdfs:subClassOf rdf:resource="#JavaSecurityCertAPI"/>
		<rdfs:subClassOf rdf:resource="#JavaSecurityInterfacesAPI"/>
		<rdfs:subClassOf rdf:resource="#JavaSecuritySpecAPI"/>
		<rdfs:subClassOf rdf:resource="#JavaSecurityAclAPI"/>
		<rdfs:subClassOf rdf:resource="#JavaNetAPI"/>
		<rdfs:subClassOf rdf:resource="#JavaUtilAPI"/>
		<rdfs:subClassOf rdf:resource="#JavaUtilJarAPI"/>
		<rdfs:subClassOf rdf:resource="#JavaUtilZipAPI"/>
		<rdfs:subClassOf rdf:resource="#JavaMathAPI"/>
		<rdfs:subClassOf rdf:resource="#JavaTextAPI"/>
		<rdfs:subClassOf rdf:resource="#JavaAwtAPI"/>
		<rdfs:subClassOf rdf:resource="#JavaAwtImAPI"/>
		<rdfs:subClassOf rdf:resource="#JavaAwtFontAPI"/>
		<rdfs:subClassOf rdf:resource="#JavaAwtEventAPI"/>
		<rdfs:subClassOf rdf:resource="#JavaAwtImageAPI"/>
		<rdfs:subClassOf rdf:resource="#JavaAwtColorAPI"/>
		<rdfs:subClassOf rdf:resource="#JavaAwtDatatransferAPI"/>
		<rdfs:subClassOf rdf:resource="#JavaBeansAPI"/>
		<rdfs:subClassOf rdf:resource="#JavaRmiAPI"/>
		<rdfs:subClassOf rdf:resource="#JavaRmiRegistryAPI"/>
		<rdfs:subClassOf rdf:resource="#JavaAppletAPI"/>
		<rdfs:subClassOf rdf:resource="#JavaxSecurityAuthX500API"/>
		<rdfs:subClassOf rdf:resource="#JavaxMicroeditionIoAPI"/>
		<rdfs:subClassOf rdf:resource="#JavaxMicroeditionPkiAPI"/>
		<rdfs:subClassOf rdf:resource="#JavaxMicroeditionXletAPI"/>
		<rdfs:subClassOf rdf:resource="#JavaxMicroeditionXletIxcAPI"/>
		<rdfs:comment xml:lang="en">J2ME PP 1.1 API</rdfs:comment>
		<rdfs:comment xml:lang="OWLManchester">platform:comprisesInterfacePart some JavaIo and platform:comprisesInterfacePart some JavaLang and platform:comprisesInterfacePart some JavaLangRef and platform:comprisesInterfacePart some JavaLangReflect and platform:comprisesInterfacePart some JavaSecurity and platform:comprisesInterfacePart some JavaSecurityCert and platform:comprisesInterfacePart some JavaSecurityInterfaces and platform:comprisesInterfacePart some JavaSecuritySpec and platform:comprisesInterfacePart some JavaSecurityAcl and platform:comprisesInterfacePart some JavaNet and platform:comprisesInterfacePart some JavaUtil and platform:comprisesInterfacePart some JavaUtilJar and platform:comprisesInterfacePart some JavaUtilZip and platform:comprisesInterfacePart some JavaMath and platform:comprisesInterfacePart some JavaText and platform:comprisesInterfacePart some JavaAwt and platform:comprisesInterfacePart some JavaAwtIm and platform:comprisesInterfacePart some JavaAwtFont and platform:comprisesInterfacePart some JavaAwtEvent and platform:comprisesInterfacePart some JavaAwtImage and platform:comprisesInterfacePart some JavaAwtColor and platform:comprisesInterfacePart some JavaAwtDatatransfer and platform:comprisesInterfacePart some JavaBeans and platform:comprisesInterfacePart some JavaRmi and platform:comprisesInterfacePart some JavaRmiRegistry and platform:comprisesInterfacePart some JavaApplet and platform:comprisesInterfacePart some JavaxSecurityAuthX500 and platform:comprisesInterfacePart some JavaxMicroeditionIo and platform:comprisesInterfacePart some JavaxMicroeditionPki and platform:comprisesInterfacePart some JavaxMicroeditionXlet and platform:comprisesInterfacePart some JavaxMicroeditionXletIxc</rdfs:comment>
	</owl:Class>
	<owl:Class rdf:about="#J2MEPP1_1ClassLibrary">
		<rdfs:subClassOf rdf:resource="#JavaIoClassLibrary"/>
		<rdfs:subClassOf rdf:resource="#JavaLangClassLibrary"/>
		<rdfs:subClassOf rdf:resource="#JavaLangRefClassLibrary"/>
		<rdfs:subClassOf rdf:resource="#JavaLangReflectClassLibrary"/>
		<rdfs:subClassOf rdf:resource="#JavaSecurityClassLibrary"/>
		<rdfs:subClassOf rdf:resource="#JavaSecurityCertClassLibrary"/>
		<rdfs:subClassOf rdf:resource="#JavaSecurityInterfacesClassLibrary"/>
		<rdfs:subClassOf rdf:resource="#JavaSecuritySpecClassLibrary"/>
		<rdfs:subClassOf rdf:resource="#JavaSecurityAclClassLibrary"/>
		<rdfs:subClassOf rdf:resource="#JavaNetClassLibrary"/>
		<rdfs:subClassOf rdf:resource="#JavaUtilClassLibrary"/>
		<rdfs:subClassOf rdf:resource="#JavaUtilJarClassLibrary"/>
		<rdfs:subClassOf rdf:resource="#JavaUtilZipClassLibrary"/>
		<rdfs:subClassOf rdf:resource="#JavaMathClassLibrary"/>
		<rdfs:subClassOf rdf:resource="#JavaTextClassLibrary"/>
		<rdfs:subClassOf rdf:resource="#JavaAwtClassLibrary"/>
		<rdfs:subClassOf rdf:resource="#JavaAwtImClassLibrary"/>
		<rdfs:subClassOf rdf:resource="#JavaAwtFontClassLibrary"/>
		<rdfs:subClassOf rdf:resource="#JavaAwtEventClassLibrary"/>
		<rdfs:subClassOf rdf:resource="#JavaAwtImageClassLibrary"/>
		<rdfs:subClassOf rdf:resource="#JavaAwtColorClassLibrary"/>
		<rdfs:subClassOf rdf:resource="#JavaAwtDatatransferClassLibrary"/>
		<rdfs:subClassOf rdf:resource="#JavaBeansClassLibrary"/>
		<rdfs:subClassOf rdf:resource="#JavaRmiClassLibrary"/>
		<rdfs:subClassOf rdf:resource="#JavaRmiRegistryClassLibrary"/>
		<rdfs:subClassOf rdf:resource="#JavaAppletClassLibrary"/>
		<rdfs:subClassOf rdf:resource="#JavaxSecurityAuthX500ClassLibrary"/>
		<rdfs:subClassOf rdf:resource="#JavaxMicroeditionIoClassLibrary"/>
		<rdfs:subClassOf rdf:resource="#JavaxMicroeditionPkiClassLibrary"/>
		<rdfs:subClassOf rdf:resource="#JavaxMicroeditionXletClassLibrary"/>
		<rdfs:subClassOf rdf:resource="#JavaxMicroeditionXletIxcClassLibrary"/>
		<rdfs:comment xml:lang="en">Java class library implementing the J2ME PP 1.1 API</rdfs:comment>
		<rdfs:comment xml:lang="OWLManchester">platform:implementsInterface some J2MEPP1_1API</rdfs:comment>
	</owl:Class>
	<owl:Class rdf:about="#J2MEPP1_1BytecodeFormat">
		<rdfs:subClassOf rdf:resource="&j2me-pp-1_0;J2MEPP1_0BytecodeFormat"/>
		<rdfs:subClassOf rdf:resource="&j2se-1_3;J2SE1_3BytecodeFormat"/>
		<rdfs:comment xml:lang="en">J2ME PP 1.1 bytecode format</rdfs:comment>
		<rdfs:comment xml:lang="OWLManchester">java:majorVersionNumber some xsd:integer[>="48"^^xsd:integer] and java:preverified value false</rdfs:comment>
	</owl:Class>
	<J2MEPP1_1BytecodeFormat rdf:about="#theJ2MEPP1_1BytecodeFormat">
		<java:preverified rdf:datatype="http://www.w3.org/2001/XMLSchema#boolean">false</java:preverified>
		<java:minorVersionNumber rdf:datatype="http://www.w3.org/2001/XMLSchema#integer">0</java:minorVersionNumber>
		<java:majorVersionNumber rdf:datatype="http://www.w3.org/2001/XMLSchema#integer">48</java:majorVersionNumber>
	</J2MEPP1_1BytecodeFormat>
	<J2MEPP1_1API rdf:about="#theJ2MEPP1_1API">
		<platform:comprisesInterfacePart rdf:resource="#theJavaxMicroeditionXletIxcPart"/>
		<platform:comprisesInterfacePart rdf:resource="#theJavaxMicroeditionXletPart"/>
		<platform:comprisesInterfacePart rdf:resource="#theJavaxMicroeditionPkiPart"/>
		<platform:comprisesInterfacePart rdf:resource="#theJavaxMicroeditionIoPart"/>
		<platform:comprisesInterfacePart rdf:resource="#theJavaxSecurityAuthX500Part"/>
		<platform:comprisesInterfacePart rdf:resource="#theJavaAppletPart"/>
		<platform:comprisesInterfacePart rdf:resource="#theJavaRmiRegistryPart"/>
		<platform:comprisesInterfacePart rdf:resource="#theJavaRmiPart"/>
		<platform:comprisesInterfacePart rdf:resource="#theJavaBeansPart"/>
		<platform:comprisesInterfacePart rdf:resource="#theJavaAwtDatatransferPart"/>
		<platform:comprisesInterfacePart rdf:resource="#theJavaAwtColorPart"/>
		<platform:comprisesInterfacePart rdf:resource="#theJavaAwtImagePart"/>
		<platform:comprisesInterfacePart rdf:resource="#theJavaAwtEventPart"/>
		<platform:comprisesInterfacePart rdf:resource="#theJavaAwtFontPart"/>
		<platform:comprisesInterfacePart rdf:resource="#theJavaAwtImPart"/>
		<platform:comprisesInterfacePart rdf:resource="#theJavaAwtPart"/>
		<platform:comprisesInterfacePart rdf:resource="#theJavaTextPart"/>
		<platform:comprisesInterfacePart rdf:resource="#theJavaMathPart"/>
		<platform:comprisesInterfacePart rdf:resource="#theJavaUtilZipPart"/>
		<platform:comprisesInterfacePart rdf:resource="#theJavaUtilJarPart"/>
		<platform:comprisesInterfacePart rdf:resource="#theJavaUtilPart"/>
		<platform:comprisesInterfacePart rdf:resource="#theJavaNetPart"/>
		<platform:comprisesInterfacePart rdf:resource="#theJavaSecurityAclPart"/>
		<platform:comprisesInterfacePart rdf:resource="#theJavaSecuritySpecPart"/>
		<platform:comprisesInterfacePart rdf:resource="#theJavaSecurityInterfacesPart"/>
		<platform:comprisesInterfacePart rdf:resource="#theJavaSecurityCertPart"/>
		<platform:comprisesInterfacePart rdf:resource="#theJavaSecurityPart"/>
		<platform:comprisesInterfacePart rdf:resource="#theJavaLangReflectPart"/>
		<platform:comprisesInterfacePart rdf:resource="#theJavaLangRefPart"/>
		<platform:comprisesInterfacePart rdf:resource="#theJavaLangPart"/>
		<platform:comprisesInterfacePart rdf:resource="#theJavaIoPart"/>
	</J2MEPP1_1API>
	<owl:Class rdf:about="#J2MEPP1_1VM">
		<owl:equivalentClass>
			<owl:Restriction>
				<owl:onProperty rdf:resource="&platform;implementsInterface"/>
				<owl:someValuesFrom rdf:resource="#J2MEPP1_1BytecodeFormat"/>
			</owl:Restriction>
		</owl:equivalentClass>
		<rdfs:subClassOf rdf:resource="&java;JavaVM"/>
		<rdfs:comment xml:lang="en">J2ME PP 1.1 virtual machine</rdfs:comment>
	</owl:Class>
	<owl:Class rdf:about="#J2MEPP1_1JRE">
		<owl:equivalentClass>
			<owl:Class >
				<owl:intersectionOf rdf:parseType="Collection">
					<owl:Restriction>
						<owl:onProperty rdf:resource="&platform;providesFeature"/>
						<owl:someValuesFrom rdf:resource="#J2MEPP1_1ClassLibrary"/>
					</owl:Restriction>
					<owl:Restriction>
						<owl:onProperty rdf:resource="&platform;providesFeature"/>
						<owl:someValuesFrom rdf:resource="#J2MEPP1_1VM"/>
					</owl:Restriction>
				</owl:intersectionOf>
			</owl:Class>
		</owl:equivalentClass>
		<rdfs:subClassOf rdf:resource="&java;JRE"/>
		<rdfs:comment xml:lang="en">J2ME PP 1.1 Java Runtime Environment</rdfs:comment>
	</owl:Class>
	<owl:Class rdf:about="#JavaIo">
		<rdfs:subClassOf rdf:resource="&j2me-pp-1_0;JavaIo"/>
		<rdfs:seeAlso rdf:resource="#JavaLang"/>
		<rdfs:seeAlso rdf:resource="#JavaNet"/>
		<rdfs:seeAlso rdf:resource="#JavaUtil"/>
		<rdfs:seeAlso rdf:resource="#JavaSecurity"/>
		<rdfs:comment xml:lang="en">Java API part implementing the java.io package for J2ME PP 1.1</rdfs:comment>
	</owl:Class>
	<owl:Class rdf:about="#JavaLang">
		<rdfs:subClassOf rdf:resource="&j2me-pp-1_0;JavaLang"/>
		<rdfs:seeAlso rdf:resource="#JavaNet"/>
		<rdfs:seeAlso rdf:resource="#JavaLangReflect"/>
		<rdfs:seeAlso rdf:resource="#JavaUtil"/>
		<rdfs:seeAlso rdf:resource="#JavaIo"/>
		<rdfs:seeAlso rdf:resource="#JavaSecurity"/>
		<rdfs:comment xml:lang="en">Java API part implementing the java.lang package for J2ME PP 1.1</rdfs:comment>
	</owl:Class>
	<owl:Class rdf:about="#JavaLangRef">
		<owl:equivalentClass rdf:resource="&j2me-pp-1_0;JavaLangRef"/>
		<owl:equivalentClass rdf:resource="&j2se-1_3;JavaLangRef"/>
		<rdfs:subClassOf rdf:resource="&java;JavaAPIPart"/>
		<rdfs:seeAlso rdf:resource="#JavaLang"/>
		<rdfs:comment xml:lang="en">Java API part implementing the java.lang.ref package for J2ME PP 1.1</rdfs:comment>
	</owl:Class>
	<owl:Class rdf:about="#JavaLangReflect">
		<rdfs:subClassOf rdf:resource="&j2me-pp-1_0;JavaLangReflect"/>
		<rdfs:subClassOf rdf:resource="&j2se-1_3;JavaLangReflect"/>
		<rdfs:seeAlso rdf:resource="#JavaLang"/>
		<rdfs:seeAlso rdf:resource="#JavaIo"/>
		<rdfs:seeAlso rdf:resource="#JavaSecurity"/>
		<rdfs:comment xml:lang="en">Java API part implementing the java.lang.reflect package for J2ME PP 1.1</rdfs:comment>
	</owl:Class>
	<owl:Class rdf:about="#JavaSecurity">
		<rdfs:subClassOf rdf:resource="&j2me-pp-1_0;JavaSecurity"/>
		<rdfs:seeAlso rdf:resource="#JavaLang"/>
		<rdfs:seeAlso rdf:resource="#JavaSecuritySpec"/>
		<rdfs:seeAlso rdf:resource="#JavaUtil"/>
		<rdfs:seeAlso rdf:resource="#JavaIo"/>
		<rdfs:seeAlso rdf:resource="#JavaNet"/>
		<rdfs:seeAlso rdf:resource="#JavaSecurityCert"/>
		<rdfs:comment xml:lang="en">Java API part implementing the java.security package for J2ME PP 1.1</rdfs:comment>
	</owl:Class>
	<owl:Class rdf:about="#JavaSecurityCert">
		<rdfs:subClassOf rdf:resource="&j2me-pp-1_0;JavaSecurityCert"/>
		<rdfs:subClassOf rdf:resource="&j2se-1_3;JavaSecurityCert"/>
		<rdfs:seeAlso rdf:resource="#JavaLang"/>
		<rdfs:seeAlso rdf:resource="#JavaxSecurityAuthX500"/>
		<rdfs:seeAlso rdf:resource="#JavaMath"/>
		<rdfs:seeAlso rdf:resource="#JavaUtil"/>
		<rdfs:seeAlso rdf:resource="#JavaIo"/>
		<rdfs:seeAlso rdf:resource="#JavaSecurity"/>
		<rdfs:comment xml:lang="en">Java API part implementing the java.security.cert package for J2ME PP 1.1</rdfs:comment>
	</owl:Class>
	<owl:Class rdf:about="#JavaSecurityInterfaces">
		<owl:equivalentClass rdf:resource="&j2me-pp-1_0;JavaSecurityInterfaces"/>
		<owl:equivalentClass rdf:resource="&j2se-1_3;JavaSecurityInterfaces"/>
		<rdfs:subClassOf rdf:resource="&java;JavaAPIPart"/>
		<rdfs:seeAlso rdf:resource="#JavaMath"/>
		<rdfs:seeAlso rdf:resource="#JavaSecurity"/>
		<rdfs:comment xml:lang="en">Java API part implementing the java.security.interfaces package for J2ME PP 1.1</rdfs:comment>
	</owl:Class>
	<owl:Class rdf:about="#JavaSecuritySpec">
		<rdfs:subClassOf rdf:resource="&j2me-pp-1_0;JavaSecuritySpec"/>
		<rdfs:subClassOf rdf:resource="&j2se-1_3;JavaSecuritySpec"/>
		<rdfs:seeAlso rdf:resource="#JavaLang"/>
		<rdfs:seeAlso rdf:resource="#JavaMath"/>
		<rdfs:seeAlso rdf:resource="#JavaSecurityInterfaces"/>
		<rdfs:seeAlso rdf:resource="#JavaSecurity"/>
		<rdfs:comment xml:lang="en">Java API part implementing the java.security.spec package for J2ME PP 1.1</rdfs:comment>
	</owl:Class>
	<owl:Class rdf:about="#JavaSecurityAcl">
		<rdfs:subClassOf rdf:resource="&j2me-pp-1_0;JavaSecurityAcl"/>
		<rdfs:subClassOf rdf:resource="&j2se-1_3;JavaSecurityAcl"/>
		<rdfs:seeAlso rdf:resource="#JavaLang"/>
		<rdfs:seeAlso rdf:resource="#JavaUtil"/>
		<rdfs:seeAlso rdf:resource="#JavaSecurity"/>
		<rdfs:comment xml:lang="en">Java API part implementing the java.security.acl package for J2ME PP 1.1</rdfs:comment>
	</owl:Class>
	<owl:Class rdf:about="#JavaNet">
		<rdfs:subClassOf rdf:resource="&j2me-pp-1_0;JavaNet"/>
		<rdfs:seeAlso rdf:resource="#JavaLang"/>
		<rdfs:seeAlso rdf:resource="#JavaUtil"/>
		<rdfs:seeAlso rdf:resource="#JavaIo"/>
		<rdfs:seeAlso rdf:resource="#JavaUtilJar"/>
		<rdfs:seeAlso rdf:resource="#JavaSecurity"/>
		<rdfs:comment xml:lang="en">Java API part implementing the java.net package for J2ME PP 1.1</rdfs:comment>
	</owl:Class>
	<owl:Class rdf:about="#JavaUtil">
		<rdfs:subClassOf rdf:resource="&j2me-pp-1_0;JavaUtil"/>
		<rdfs:seeAlso rdf:resource="#JavaLang"/>
		<rdfs:seeAlso rdf:resource="#JavaIo"/>
		<rdfs:seeAlso rdf:resource="#JavaSecurity"/>
		<rdfs:comment xml:lang="en">Java API part implementing the java.util package for J2ME PP 1.1</rdfs:comment>
	</owl:Class>
	<owl:Class rdf:about="#JavaUtilJar">
		<rdfs:subClassOf rdf:resource="&j2me-pp-1_0;JavaUtilJar"/>
		<rdfs:subClassOf rdf:resource="&j2se-1_3;JavaUtilJar"/>
		<rdfs:seeAlso rdf:resource="#JavaLang"/>
		<rdfs:seeAlso rdf:resource="#JavaUtilZip"/>
		<rdfs:seeAlso rdf:resource="#JavaUtil"/>
		<rdfs:seeAlso rdf:resource="#JavaIo"/>
		<rdfs:comment xml:lang="en">Java API part implementing the java.util.jar package for J2ME PP 1.1</rdfs:comment>
	</owl:Class>
	<owl:Class rdf:about="#JavaUtilZip">
		<rdfs:subClassOf rdf:resource="&j2me-pp-1_0;JavaUtilZip"/>
		<rdfs:subClassOf rdf:resource="&j2se-1_3;JavaUtilZip"/>
		<rdfs:seeAlso rdf:resource="#JavaLang"/>
		<rdfs:seeAlso rdf:resource="#JavaUtil"/>
		<rdfs:seeAlso rdf:resource="#JavaIo"/>
		<rdfs:comment xml:lang="en">Java API part implementing the java.util.zip package for J2ME PP 1.1</rdfs:comment>
	</owl:Class>
	<owl:Class rdf:about="#JavaMath">
		<owl:equivalentClass rdf:resource="&j2me-pp-1_0;JavaMath"/>
		<owl:equivalentClass rdf:resource="&j2se-1_3;JavaMath"/>
		<rdfs:subClassOf rdf:resource="&java;JavaAPIPart"/>
		<rdfs:seeAlso rdf:resource="#JavaLang"/>
		<rdfs:seeAlso rdf:resource="#JavaUtil"/>
		<rdfs:comment xml:lang="en">Java API part implementing the java.math package for J2ME PP 1.1</rdfs:comment>
	</owl:Class>
	<owl:Class rdf:about="#JavaText">
		<rdfs:subClassOf rdf:resource="&j2me-pp-1_0;JavaText"/>
		<rdfs:subClassOf rdf:resource="&j2se-1_3;JavaText"/>
		<rdfs:seeAlso rdf:resource="#JavaLang"/>
		<rdfs:seeAlso rdf:resource="#JavaUtil"/>
		<rdfs:seeAlso rdf:resource="#JavaIo"/>
		<rdfs:comment xml:lang="en">Java API part implementing the java.text package for J2ME PP 1.1</rdfs:comment>
	</owl:Class>
	<owl:Class rdf:about="#JavaAwt">
		<rdfs:subClassOf rdf:resource="&j2me-pp-1_0;JavaAwt"/>
		<rdfs:seeAlso rdf:resource="#JavaAwtDatatransfer"/>
		<rdfs:seeAlso rdf:resource="#JavaBeans"/>
		<rdfs:seeAlso rdf:resource="#JavaText"/>
		<rdfs:seeAlso rdf:resource="#JavaUtil"/>
		<rdfs:seeAlso rdf:resource="#JavaIo"/>
		<rdfs:seeAlso rdf:resource="#JavaAwtEvent"/>
		<rdfs:seeAlso rdf:resource="#JavaAwtIm"/>
		<rdfs:seeAlso rdf:resource="#JavaLang"/>
		<rdfs:seeAlso rdf:resource="#JavaAwtColor"/>
		<rdfs:seeAlso rdf:resource="#JavaNet"/>
		<rdfs:seeAlso rdf:resource="#JavaAwtImage"/>
		<rdfs:seeAlso rdf:resource="#JavaSecurity"/>
		<rdfs:comment xml:lang="en">Java API part implementing the java.awt package for J2ME PP 1.1</rdfs:comment>
	</owl:Class>
	<owl:Class rdf:about="#JavaAwtIm">
		<rdfs:subClassOf rdf:resource="&java;JavaAPIPart"/>
		<rdfs:seeAlso rdf:resource="#JavaAwt"/>
		<rdfs:seeAlso rdf:resource="#JavaLang"/>
		<rdfs:seeAlso rdf:resource="#JavaUtil"/>
		<rdfs:seeAlso rdf:resource="#JavaAwtFont"/>
		<rdfs:seeAlso rdf:resource="#JavaText"/>
		<rdfs:comment xml:lang="en">Java API part implementing the java.awt.im package for J2ME PP 1.1</rdfs:comment>
	</owl:Class>
	<owl:Class rdf:about="#JavaAwtFont">
		<rdfs:subClassOf rdf:resource="&java;JavaAPIPart"/>
		<rdfs:seeAlso rdf:resource="#JavaLang"/>
		<rdfs:seeAlso rdf:resource="#JavaText"/>
		<rdfs:comment xml:lang="en">Java API part implementing the java.awt.font package for J2ME PP 1.1</rdfs:comment>
	</owl:Class>
	<owl:Class rdf:about="#JavaAwtEvent">
		<rdfs:subClassOf rdf:resource="&j2me-pp-1_0;JavaAwtEvent"/>
		<rdfs:seeAlso rdf:resource="#JavaAwt"/>
		<rdfs:seeAlso rdf:resource="#JavaLang"/>
		<rdfs:seeAlso rdf:resource="#JavaAwtFont"/>
		<rdfs:seeAlso rdf:resource="#JavaText"/>
		<rdfs:seeAlso rdf:resource="#JavaUtil"/>
		<rdfs:comment xml:lang="en">Java API part implementing the java.awt.event package for J2ME PP 1.1</rdfs:comment>
	</owl:Class>
	<owl:Class rdf:about="#JavaAwtImage">
		<rdfs:subClassOf rdf:resource="&j2me-pp-1_0;JavaAwtImage"/>
		<rdfs:seeAlso rdf:resource="#JavaAwt"/>
		<rdfs:seeAlso rdf:resource="#JavaAwtColor"/>
		<rdfs:seeAlso rdf:resource="#JavaLang"/>
		<rdfs:seeAlso rdf:resource="#JavaUtil"/>
		<rdfs:comment xml:lang="en">Java API part implementing the java.awt.image package for J2ME PP 1.1</rdfs:comment>
	</owl:Class>
	<owl:Class rdf:about="#JavaAwtColor">
		<owl:equivalentClass rdf:resource="&j2me-pp-1_0;JavaAwtColor"/>
		<rdfs:subClassOf rdf:resource="&java;JavaAPIPart"/>
		<rdfs:seeAlso rdf:resource="#JavaLang"/>
		<rdfs:seeAlso rdf:resource="#JavaIo"/>
		<rdfs:comment xml:lang="en">Java API part implementing the java.awt.color package for J2ME PP 1.1</rdfs:comment>
	</owl:Class>
	<owl:Class rdf:about="#JavaAwtDatatransfer">
		<rdfs:subClassOf rdf:resource="&j2me-pp-1_0;JavaAwtDatatransfer"/>
		<rdfs:seeAlso rdf:resource="#JavaLang"/>
		<rdfs:seeAlso rdf:resource="#JavaIo"/>
		<rdfs:comment xml:lang="en">Java API part implementing the java.awt.datatransfer package for J2ME PP 1.1</rdfs:comment>
	</owl:Class>
	<owl:Class rdf:about="#JavaBeans">
		<rdfs:subClassOf rdf:resource="&j2me-pp-1_0;JavaBeans"/>
		<rdfs:seeAlso rdf:resource="#JavaLang"/>
		<rdfs:seeAlso rdf:resource="#JavaUtil"/>
		<rdfs:seeAlso rdf:resource="#JavaIo"/>
		<rdfs:comment xml:lang="en">Java API part implementing the java.beans package for J2ME PP 1.1</rdfs:comment>
	</owl:Class>
	<owl:Class rdf:about="#JavaRmi">
		<rdfs:subClassOf rdf:resource="&j2me-pp-1_0;JavaRmi"/>
		<rdfs:seeAlso rdf:resource="#JavaLang"/>
		<rdfs:seeAlso rdf:resource="#JavaIo"/>
		<rdfs:comment xml:lang="en">Java API part implementing the java.rmi package for J2ME PP 1.1</rdfs:comment>
	</owl:Class>
	<owl:Class rdf:about="#JavaRmiRegistry">
		<owl:equivalentClass rdf:resource="&j2me-pp-1_0;JavaRmiRegistry"/>
		<rdfs:subClassOf rdf:resource="&java;JavaAPIPart"/>
		<rdfs:seeAlso rdf:resource="#JavaLang"/>
		<rdfs:seeAlso rdf:resource="#JavaRmi"/>
		<rdfs:comment xml:lang="en">Java API part implementing the java.rmi.registry package for J2ME PP 1.1</rdfs:comment>
	</owl:Class>
	<owl:Class rdf:about="#JavaApplet">
		<rdfs:subClassOf rdf:resource="&j2me-pp-1_0;JavaApplet"/>
		<rdfs:seeAlso rdf:resource="#JavaAwt"/>
		<rdfs:seeAlso rdf:resource="#JavaLang"/>
		<rdfs:seeAlso rdf:resource="#JavaUtil"/>
		<rdfs:seeAlso rdf:resource="#JavaNet"/>
		<rdfs:comment xml:lang="en">Java API part implementing the java.applet package for J2ME PP 1.1</rdfs:comment>
	</owl:Class>
	<owl:Class rdf:about="#JavaxSecurityAuthX500">
		<rdfs:subClassOf rdf:resource="&java;JavaAPIPart"/>
		<rdfs:seeAlso rdf:resource="#JavaLang"/>
		<rdfs:seeAlso rdf:resource="#JavaIo"/>
		<rdfs:seeAlso rdf:resource="#JavaSecurity"/>
		<rdfs:comment xml:lang="en">Java API part implementing the javax.security.auth.x500 package for J2ME PP 1.1</rdfs:comment>
	</owl:Class>
	<owl:Class rdf:about="#JavaxMicroeditionIo">
		<rdfs:subClassOf rdf:resource="&j2me-pp-1_0;JavaxMicroeditionIo"/>
		<rdfs:seeAlso rdf:resource="#JavaLang"/>
		<rdfs:seeAlso rdf:resource="#JavaIo"/>
		<rdfs:seeAlso rdf:resource="#JavaxMicroeditionPki"/>
		<rdfs:comment xml:lang="en">Java API part implementing the javax.microedition.io package for J2ME PP 1.1</rdfs:comment>
	</owl:Class>
	<owl:Class rdf:about="#JavaxMicroeditionPki">
		<rdfs:subClassOf rdf:resource="&java;JavaAPIPart"/>
		<rdfs:seeAlso rdf:resource="#JavaLang"/>
		<rdfs:seeAlso rdf:resource="#JavaIo"/>
		<rdfs:comment xml:lang="en">Java API part implementing the javax.microedition.pki package for J2ME PP 1.1</rdfs:comment>
	</owl:Class>
	<owl:Class rdf:about="#JavaxMicroeditionXlet">
		<rdfs:subClassOf rdf:resource="&j2me-pp-1_0;JavaxMicroeditionXlet"/>
		<rdfs:seeAlso rdf:resource="#JavaAwt"/>
		<rdfs:seeAlso rdf:resource="#JavaLang"/>
		<rdfs:comment xml:lang="en">Java API part implementing the javax.microedition.xlet package for J2ME PP 1.1</rdfs:comment>
	</owl:Class>
	<owl:Class rdf:about="#JavaxMicroeditionXletIxc">
		<rdfs:subClassOf rdf:resource="&j2me-pp-1_0;JavaxMicroeditionXletIxc"/>
		<rdfs:seeAlso rdf:resource="#JavaxMicroeditionXlet"/>
		<rdfs:seeAlso rdf:resource="#JavaLang"/>
		<rdfs:seeAlso rdf:resource="#JavaRmi"/>
		<rdfs:seeAlso rdf:resource="#JavaRmiRegistry"/>
		<rdfs:seeAlso rdf:resource="#JavaSecurity"/>
		<rdfs:comment xml:lang="en">Java API part implementing the javax.microedition.xlet.ixc package for J2ME PP 1.1</rdfs:comment>
	</owl:Class>
	<owl:Class rdf:about="#JavaIoAPI">
		<rdfs:subClassOf rdf:resource="&j2me-pp-1_0;JavaIoAPI"/>
		<rdfs:comment xml:lang="en">JavaLibrary implementing the java.io package for J2ME PP 1.1</rdfs:comment>
		<rdfs:comment xml:lang="OWLManchester">platform:comprisesInterfacePart some JavaIo</rdfs:comment>
	</owl:Class>
	<owl:Class rdf:about="#JavaLangAPI">
		<rdfs:subClassOf rdf:resource="&j2me-pp-1_0;JavaLangAPI"/>
		<rdfs:comment xml:lang="en">JavaLibrary implementing the java.lang package for J2ME PP 1.1</rdfs:comment>
		<rdfs:comment xml:lang="OWLManchester">platform:comprisesInterfacePart some JavaLang</rdfs:comment>
	</owl:Class>
	<owl:Class rdf:about="#JavaLangRefAPI">
		<owl:equivalentClass rdf:resource="&j2me-pp-1_0;JavaLangRefAPI"/>
		<owl:equivalentClass rdf:resource="&j2se-1_3;JavaLangRefAPI"/>
		<rdfs:subClassOf rdf:resource="&java;JavaAPI"/>
		<rdfs:comment xml:lang="en">JavaLibrary implementing the java.lang.ref package for J2ME PP 1.1</rdfs:comment>
		<rdfs:comment xml:lang="OWLManchester">platform:comprisesInterfacePart some JavaLangRef</rdfs:comment>
	</owl:Class>
	<owl:Class rdf:about="#JavaLangReflectAPI">
		<rdfs:subClassOf rdf:resource="&j2me-pp-1_0;JavaLangReflectAPI"/>
		<rdfs:subClassOf rdf:resource="&j2se-1_3;JavaLangReflectAPI"/>
		<rdfs:comment xml:lang="en">JavaLibrary implementing the java.lang.reflect package for J2ME PP 1.1</rdfs:comment>
		<rdfs:comment xml:lang="OWLManchester">platform:comprisesInterfacePart some JavaLangReflect</rdfs:comment>
	</owl:Class>
	<owl:Class rdf:about="#JavaSecurityAPI">
		<rdfs:subClassOf rdf:resource="&j2me-pp-1_0;JavaSecurityAPI"/>
		<rdfs:comment xml:lang="en">JavaLibrary implementing the java.security package for J2ME PP 1.1</rdfs:comment>
		<rdfs:comment xml:lang="OWLManchester">platform:comprisesInterfacePart some JavaSecurity</rdfs:comment>
	</owl:Class>
	<owl:Class rdf:about="#JavaSecurityCertAPI">
		<rdfs:subClassOf rdf:resource="&j2me-pp-1_0;JavaSecurityCertAPI"/>
		<rdfs:subClassOf rdf:resource="&j2se-1_3;JavaSecurityCertAPI"/>
		<rdfs:comment xml:lang="en">JavaLibrary implementing the java.security.cert package for J2ME PP 1.1</rdfs:comment>
		<rdfs:comment xml:lang="OWLManchester">platform:comprisesInterfacePart some JavaSecurityCert</rdfs:comment>
	</owl:Class>
	<owl:Class rdf:about="#JavaSecurityInterfacesAPI">
		<owl:equivalentClass rdf:resource="&j2me-pp-1_0;JavaSecurityInterfacesAPI"/>
		<owl:equivalentClass rdf:resource="&j2se-1_3;JavaSecurityInterfacesAPI"/>
		<rdfs:subClassOf rdf:resource="&java;JavaAPI"/>
		<rdfs:comment xml:lang="en">JavaLibrary implementing the java.security.interfaces package for J2ME PP 1.1</rdfs:comment>
		<rdfs:comment xml:lang="OWLManchester">platform:comprisesInterfacePart some JavaSecurityInterfaces</rdfs:comment>
	</owl:Class>
	<owl:Class rdf:about="#JavaSecuritySpecAPI">
		<rdfs:subClassOf rdf:resource="&j2me-pp-1_0;JavaSecuritySpecAPI"/>
		<rdfs:subClassOf rdf:resource="&j2se-1_3;JavaSecuritySpecAPI"/>
		<rdfs:comment xml:lang="en">JavaLibrary implementing the java.security.spec package for J2ME PP 1.1</rdfs:comment>
		<rdfs:comment xml:lang="OWLManchester">platform:comprisesInterfacePart some JavaSecuritySpec</rdfs:comment>
	</owl:Class>
	<owl:Class rdf:about="#JavaSecurityAclAPI">
		<rdfs:subClassOf rdf:resource="&j2me-pp-1_0;JavaSecurityAclAPI"/>
		<rdfs:subClassOf rdf:resource="&j2se-1_3;JavaSecurityAclAPI"/>
		<rdfs:comment xml:lang="en">JavaLibrary implementing the java.security.acl package for J2ME PP 1.1</rdfs:comment>
		<rdfs:comment xml:lang="OWLManchester">platform:comprisesInterfacePart some JavaSecurityAcl</rdfs:comment>
	</owl:Class>
	<owl:Class rdf:about="#JavaNetAPI">
		<rdfs:subClassOf rdf:resource="&j2me-pp-1_0;JavaNetAPI"/>
		<rdfs:comment xml:lang="en">JavaLibrary implementing the java.net package for J2ME PP 1.1</rdfs:comment>
		<rdfs:comment xml:lang="OWLManchester">platform:comprisesInterfacePart some JavaNet</rdfs:comment>
	</owl:Class>
	<owl:Class rdf:about="#JavaUtilAPI">
		<rdfs:subClassOf rdf:resource="&j2me-pp-1_0;JavaUtilAPI"/>
		<rdfs:comment xml:lang="en">JavaLibrary implementing the java.util package for J2ME PP 1.1</rdfs:comment>
		<rdfs:comment xml:lang="OWLManchester">platform:comprisesInterfacePart some JavaUtil</rdfs:comment>
	</owl:Class>
	<owl:Class rdf:about="#JavaUtilJarAPI">
		<rdfs:subClassOf rdf:resource="&j2me-pp-1_0;JavaUtilJarAPI"/>
		<rdfs:subClassOf rdf:resource="&j2se-1_3;JavaUtilJarAPI"/>
		<rdfs:comment xml:lang="en">JavaLibrary implementing the java.util.jar package for J2ME PP 1.1</rdfs:comment>
		<rdfs:comment xml:lang="OWLManchester">platform:comprisesInterfacePart some JavaUtilJar</rdfs:comment>
	</owl:Class>
	<owl:Class rdf:about="#JavaUtilZipAPI">
		<rdfs:subClassOf rdf:resource="&j2me-pp-1_0;JavaUtilZipAPI"/>
		<rdfs:subClassOf rdf:resource="&j2se-1_3;JavaUtilZipAPI"/>
		<rdfs:comment xml:lang="en">JavaLibrary implementing the java.util.zip package for J2ME PP 1.1</rdfs:comment>
		<rdfs:comment xml:lang="OWLManchester">platform:comprisesInterfacePart some JavaUtilZip</rdfs:comment>
	</owl:Class>
	<owl:Class rdf:about="#JavaMathAPI">
		<owl:equivalentClass rdf:resource="&j2me-pp-1_0;JavaMathAPI"/>
		<owl:equivalentClass rdf:resource="&j2se-1_3;JavaMathAPI"/>
		<rdfs:subClassOf rdf:resource="&java;JavaAPI"/>
		<rdfs:comment xml:lang="en">JavaLibrary implementing the java.math package for J2ME PP 1.1</rdfs:comment>
		<rdfs:comment xml:lang="OWLManchester">platform:comprisesInterfacePart some JavaMath</rdfs:comment>
	</owl:Class>
	<owl:Class rdf:about="#JavaTextAPI">
		<rdfs:subClassOf rdf:resource="&j2me-pp-1_0;JavaTextAPI"/>
		<rdfs:subClassOf rdf:resource="&j2se-1_3;JavaTextAPI"/>
		<rdfs:comment xml:lang="en">JavaLibrary implementing the java.text package for J2ME PP 1.1</rdfs:comment>
		<rdfs:comment xml:lang="OWLManchester">platform:comprisesInterfacePart some JavaText</rdfs:comment>
	</owl:Class>
	<owl:Class rdf:about="#JavaAwtAPI">
		<rdfs:subClassOf rdf:resource="&j2me-pp-1_0;JavaAwtAPI"/>
		<rdfs:comment xml:lang="en">JavaLibrary implementing the java.awt package for J2ME PP 1.1</rdfs:comment>
		<rdfs:comment xml:lang="OWLManchester">platform:comprisesInterfacePart some JavaAwt</rdfs:comment>
	</owl:Class>
	<owl:Class rdf:about="#JavaAwtImAPI">
		<rdfs:subClassOf rdf:resource="&java;JavaAPI"/>
		<rdfs:comment xml:lang="en">JavaLibrary implementing the java.awt.im package for J2ME PP 1.1</rdfs:comment>
		<rdfs:comment xml:lang="OWLManchester">platform:comprisesInterfacePart some JavaAwtIm</rdfs:comment>
	</owl:Class>
	<owl:Class rdf:about="#JavaAwtFontAPI">
		<rdfs:subClassOf rdf:resource="&java;JavaAPI"/>
		<rdfs:comment xml:lang="en">JavaLibrary implementing the java.awt.font package for J2ME PP 1.1</rdfs:comment>
		<rdfs:comment xml:lang="OWLManchester">platform:comprisesInterfacePart some JavaAwtFont</rdfs:comment>
	</owl:Class>
	<owl:Class rdf:about="#JavaAwtEventAPI">
		<rdfs:subClassOf rdf:resource="&j2me-pp-1_0;JavaAwtEventAPI"/>
		<rdfs:comment xml:lang="en">JavaLibrary implementing the java.awt.event package for J2ME PP 1.1</rdfs:comment>
		<rdfs:comment xml:lang="OWLManchester">platform:comprisesInterfacePart some JavaAwtEvent</rdfs:comment>
	</owl:Class>
	<owl:Class rdf:about="#JavaAwtImageAPI">
		<rdfs:subClassOf rdf:resource="&j2me-pp-1_0;JavaAwtImageAPI"/>
		<rdfs:comment xml:lang="en">JavaLibrary implementing the java.awt.image package for J2ME PP 1.1</rdfs:comment>
		<rdfs:comment xml:lang="OWLManchester">platform:comprisesInterfacePart some JavaAwtImage</rdfs:comment>
	</owl:Class>
	<owl:Class rdf:about="#JavaAwtColorAPI">
		<owl:equivalentClass rdf:resource="&j2me-pp-1_0;JavaAwtColorAPI"/>
		<rdfs:subClassOf rdf:resource="&java;JavaAPI"/>
		<rdfs:comment xml:lang="en">JavaLibrary implementing the java.awt.color package for J2ME PP 1.1</rdfs:comment>
		<rdfs:comment xml:lang="OWLManchester">platform:comprisesInterfacePart some JavaAwtColor</rdfs:comment>
	</owl:Class>
	<owl:Class rdf:about="#JavaAwtDatatransferAPI">
		<rdfs:subClassOf rdf:resource="&j2me-pp-1_0;JavaAwtDatatransferAPI"/>
		<rdfs:comment xml:lang="en">JavaLibrary implementing the java.awt.datatransfer package for J2ME PP 1.1</rdfs:comment>
		<rdfs:comment xml:lang="OWLManchester">platform:comprisesInterfacePart some JavaAwtDatatransfer</rdfs:comment>
	</owl:Class>
	<owl:Class rdf:about="#JavaBeansAPI">
		<rdfs:subClassOf rdf:resource="&j2me-pp-1_0;JavaBeansAPI"/>
		<rdfs:comment xml:lang="en">JavaLibrary implementing the java.beans package for J2ME PP 1.1</rdfs:comment>
		<rdfs:comment xml:lang="OWLManchester">platform:comprisesInterfacePart some JavaBeans</rdfs:comment>
	</owl:Class>
	<owl:Class rdf:about="#JavaRmiAPI">
		<rdfs:subClassOf rdf:resource="&j2me-pp-1_0;JavaRmiAPI"/>
		<rdfs:comment xml:lang="en">JavaLibrary implementing the java.rmi package for J2ME PP 1.1</rdfs:comment>
		<rdfs:comment xml:lang="OWLManchester">platform:comprisesInterfacePart some JavaRmi</rdfs:comment>
	</owl:Class>
	<owl:Class rdf:about="#JavaRmiRegistryAPI">
		<owl:equivalentClass rdf:resource="&j2me-pp-1_0;JavaRmiRegistryAPI"/>
		<rdfs:subClassOf rdf:resource="&java;JavaAPI"/>
		<rdfs:comment xml:lang="en">JavaLibrary implementing the java.rmi.registry package for J2ME PP 1.1</rdfs:comment>
		<rdfs:comment xml:lang="OWLManchester">platform:comprisesInterfacePart some JavaRmiRegistry</rdfs:comment>
	</owl:Class>
	<owl:Class rdf:about="#JavaAppletAPI">
		<rdfs:subClassOf rdf:resource="&j2me-pp-1_0;JavaAppletAPI"/>
		<rdfs:comment xml:lang="en">JavaLibrary implementing the java.applet package for J2ME PP 1.1</rdfs:comment>
		<rdfs:comment xml:lang="OWLManchester">platform:comprisesInterfacePart some JavaApplet</rdfs:comment>
	</owl:Class>
	<owl:Class rdf:about="#JavaxSecurityAuthX500API">
		<rdfs:subClassOf rdf:resource="&java;JavaAPI"/>
		<rdfs:comment xml:lang="en">JavaLibrary implementing the javax.security.auth.x500 package for J2ME PP 1.1</rdfs:comment>
		<rdfs:comment xml:lang="OWLManchester">platform:comprisesInterfacePart some JavaxSecurityAuthX500</rdfs:comment>
	</owl:Class>
	<owl:Class rdf:about="#JavaxMicroeditionIoAPI">
		<rdfs:subClassOf rdf:resource="&j2me-pp-1_0;JavaxMicroeditionIoAPI"/>
		<rdfs:comment xml:lang="en">JavaLibrary implementing the javax.microedition.io package for J2ME PP 1.1</rdfs:comment>
		<rdfs:comment xml:lang="OWLManchester">platform:comprisesInterfacePart some JavaxMicroeditionIo</rdfs:comment>
	</owl:Class>
	<owl:Class rdf:about="#JavaxMicroeditionPkiAPI">
		<rdfs:subClassOf rdf:resource="&java;JavaAPI"/>
		<rdfs:comment xml:lang="en">JavaLibrary implementing the javax.microedition.pki package for J2ME PP 1.1</rdfs:comment>
		<rdfs:comment xml:lang="OWLManchester">platform:comprisesInterfacePart some JavaxMicroeditionPki</rdfs:comment>
	</owl:Class>
	<owl:Class rdf:about="#JavaxMicroeditionXletAPI">
		<rdfs:subClassOf rdf:resource="&j2me-pp-1_0;JavaxMicroeditionXletAPI"/>
		<rdfs:comment xml:lang="en">JavaLibrary implementing the javax.microedition.xlet package for J2ME PP 1.1</rdfs:comment>
		<rdfs:comment xml:lang="OWLManchester">platform:comprisesInterfacePart some JavaxMicroeditionXlet</rdfs:comment>
	</owl:Class>
	<owl:Class rdf:about="#JavaxMicroeditionXletIxcAPI">
		<rdfs:subClassOf rdf:resource="&j2me-pp-1_0;JavaxMicroeditionXletIxcAPI"/>
		<rdfs:comment xml:lang="en">JavaLibrary implementing the javax.microedition.xlet.ixc package for J2ME PP 1.1</rdfs:comment>
		<rdfs:comment xml:lang="OWLManchester">platform:comprisesInterfacePart some JavaxMicroeditionXletIxc</rdfs:comment>
	</owl:Class>
	<JavaIo rdf:about="#theJavaIoPart">
	</JavaIo>
	<JavaLang rdf:about="#theJavaLangPart">
	</JavaLang>
	<JavaLangRef rdf:about="#theJavaLangRefPart">
	</JavaLangRef>
	<JavaLangReflect rdf:about="#theJavaLangReflectPart">
	</JavaLangReflect>
	<JavaSecurity rdf:about="#theJavaSecurityPart">
	</JavaSecurity>
	<JavaSecurityCert rdf:about="#theJavaSecurityCertPart">
	</JavaSecurityCert>
	<JavaSecurityInterfaces rdf:about="#theJavaSecurityInterfacesPart">
	</JavaSecurityInterfaces>
	<JavaSecuritySpec rdf:about="#theJavaSecuritySpecPart">
	</JavaSecuritySpec>
	<JavaSecurityAcl rdf:about="#theJavaSecurityAclPart">
	</JavaSecurityAcl>
	<JavaNet rdf:about="#theJavaNetPart">
	</JavaNet>
	<JavaUtil rdf:about="#theJavaUtilPart">
	</JavaUtil>
	<JavaUtilJar rdf:about="#theJavaUtilJarPart">
	</JavaUtilJar>
	<JavaUtilZip rdf:about="#theJavaUtilZipPart">
	</JavaUtilZip>
	<JavaMath rdf:about="#theJavaMathPart">
	</JavaMath>
	<JavaText rdf:about="#theJavaTextPart">
	</JavaText>
	<JavaAwt rdf:about="#theJavaAwtPart">
	</JavaAwt>
	<JavaAwtIm rdf:about="#theJavaAwtImPart">
	</JavaAwtIm>
	<JavaAwtFont rdf:about="#theJavaAwtFontPart">
	</JavaAwtFont>
	<JavaAwtEvent rdf:about="#theJavaAwtEventPart">
	</JavaAwtEvent>
	<JavaAwtImage rdf:about="#theJavaAwtImagePart">
	</JavaAwtImage>
	<JavaAwtColor rdf:about="#theJavaAwtColorPart">
	</JavaAwtColor>
	<JavaAwtDatatransfer rdf:about="#theJavaAwtDatatransferPart">
	</JavaAwtDatatransfer>
	<JavaBeans rdf:about="#theJavaBeansPart">
	</JavaBeans>
	<JavaRmi rdf:about="#theJavaRmiPart">
	</JavaRmi>
	<JavaRmiRegistry rdf:about="#theJavaRmiRegistryPart">
	</JavaRmiRegistry>
	<JavaApplet rdf:about="#theJavaAppletPart">
	</JavaApplet>
	<JavaxSecurityAuthX500 rdf:about="#theJavaxSecurityAuthX500Part">
	</JavaxSecurityAuthX500>
	<JavaxMicroeditionIo rdf:about="#theJavaxMicroeditionIoPart">
	</JavaxMicroeditionIo>
	<JavaxMicroeditionPki rdf:about="#theJavaxMicroeditionPkiPart">
	</JavaxMicroeditionPki>
	<JavaxMicroeditionXlet rdf:about="#theJavaxMicroeditionXletPart">
	</JavaxMicroeditionXlet>
	<JavaxMicroeditionXletIxc rdf:about="#theJavaxMicroeditionXletIxcPart">
	</JavaxMicroeditionXletIxc>
	<owl:Class rdf:about="#JavaIoClassLibrary">
		<rdfs:subClassOf rdf:resource="&j2me-pp-1_0;JavaIoClassLibrary"/>
		<rdfs:comment xml:lang="en">JavaLibrary implementing the java.io package for J2ME PP 1.1</rdfs:comment>
		<rdfs:comment xml:lang="OWLManchester">platform:implementsInterface some JavaIoAPI</rdfs:comment>
	</owl:Class>
	<owl:Class rdf:about="#JavaLangClassLibrary">
		<rdfs:subClassOf rdf:resource="&j2me-pp-1_0;JavaLangClassLibrary"/>
		<rdfs:comment xml:lang="en">JavaLibrary implementing the java.lang package for J2ME PP 1.1</rdfs:comment>
		<rdfs:comment xml:lang="OWLManchester">platform:implementsInterface some JavaLangAPI</rdfs:comment>
	</owl:Class>
	<owl:Class rdf:about="#JavaLangRefClassLibrary">
		<owl:equivalentClass rdf:resource="&j2me-pp-1_0;JavaLangRefClassLibrary"/>
		<owl:equivalentClass rdf:resource="&j2se-1_3;JavaLangRefClassLibrary"/>
		<rdfs:subClassOf rdf:resource="&java;JavaClassLibrary"/>
		<rdfs:comment xml:lang="en">JavaLibrary implementing the java.lang.ref package for J2ME PP 1.1</rdfs:comment>
		<rdfs:comment xml:lang="OWLManchester">platform:implementsInterface some JavaLangRefAPI</rdfs:comment>
	</owl:Class>
	<owl:Class rdf:about="#JavaLangReflectClassLibrary">
		<rdfs:subClassOf rdf:resource="&j2me-pp-1_0;JavaLangReflectClassLibrary"/>
		<rdfs:subClassOf rdf:resource="&j2se-1_3;JavaLangReflectClassLibrary"/>
		<rdfs:comment xml:lang="en">JavaLibrary implementing the java.lang.reflect package for J2ME PP 1.1</rdfs:comment>
		<rdfs:comment xml:lang="OWLManchester">platform:implementsInterface some JavaLangReflectAPI</rdfs:comment>
	</owl:Class>
	<owl:Class rdf:about="#JavaSecurityClassLibrary">
		<rdfs:subClassOf rdf:resource="&j2me-pp-1_0;JavaSecurityClassLibrary"/>
		<rdfs:comment xml:lang="en">JavaLibrary implementing the java.security package for J2ME PP 1.1</rdfs:comment>
		<rdfs:comment xml:lang="OWLManchester">platform:implementsInterface some JavaSecurityAPI</rdfs:comment>
	</owl:Class>
	<owl:Class rdf:about="#JavaSecurityCertClassLibrary">
		<rdfs:subClassOf rdf:resource="&j2me-pp-1_0;JavaSecurityCertClassLibrary"/>
		<rdfs:subClassOf rdf:resource="&j2se-1_3;JavaSecurityCertClassLibrary"/>
		<rdfs:comment xml:lang="en">JavaLibrary implementing the java.security.cert package for J2ME PP 1.1</rdfs:comment>
		<rdfs:comment xml:lang="OWLManchester">platform:implementsInterface some JavaSecurityCertAPI</rdfs:comment>
	</owl:Class>
	<owl:Class rdf:about="#JavaSecurityInterfacesClassLibrary">
		<owl:equivalentClass rdf:resource="&j2me-pp-1_0;JavaSecurityInterfacesClassLibrary"/>
		<owl:equivalentClass rdf:resource="&j2se-1_3;JavaSecurityInterfacesClassLibrary"/>
		<rdfs:subClassOf rdf:resource="&java;JavaClassLibrary"/>
		<rdfs:comment xml:lang="en">JavaLibrary implementing the java.security.interfaces package for J2ME PP 1.1</rdfs:comment>
		<rdfs:comment xml:lang="OWLManchester">platform:implementsInterface some JavaSecurityInterfacesAPI</rdfs:comment>
	</owl:Class>
	<owl:Class rdf:about="#JavaSecuritySpecClassLibrary">
		<rdfs:subClassOf rdf:resource="&j2me-pp-1_0;JavaSecuritySpecClassLibrary"/>
		<rdfs:subClassOf rdf:resource="&j2se-1_3;JavaSecuritySpecClassLibrary"/>
		<rdfs:comment xml:lang="en">JavaLibrary implementing the java.security.spec package for J2ME PP 1.1</rdfs:comment>
		<rdfs:comment xml:lang="OWLManchester">platform:implementsInterface some JavaSecuritySpecAPI</rdfs:comment>
	</owl:Class>
	<owl:Class rdf:about="#JavaSecurityAclClassLibrary">
		<rdfs:subClassOf rdf:resource="&j2me-pp-1_0;JavaSecurityAclClassLibrary"/>
		<rdfs:subClassOf rdf:resource="&j2se-1_3;JavaSecurityAclClassLibrary"/>
		<rdfs:comment xml:lang="en">JavaLibrary implementing the java.security.acl package for J2ME PP 1.1</rdfs:comment>
		<rdfs:comment xml:lang="OWLManchester">platform:implementsInterface some JavaSecurityAclAPI</rdfs:comment>
	</owl:Class>
	<owl:Class rdf:about="#JavaNetClassLibrary">
		<rdfs:subClassOf rdf:resource="&j2me-pp-1_0;JavaNetClassLibrary"/>
		<rdfs:comment xml:lang="en">JavaLibrary implementing the java.net package for J2ME PP 1.1</rdfs:comment>
		<rdfs:comment xml:lang="OWLManchester">platform:implementsInterface some JavaNetAPI</rdfs:comment>
	</owl:Class>
	<owl:Class rdf:about="#JavaUtilClassLibrary">
		<rdfs:subClassOf rdf:resource="&j2me-pp-1_0;JavaUtilClassLibrary"/>
		<rdfs:comment xml:lang="en">JavaLibrary implementing the java.util package for J2ME PP 1.1</rdfs:comment>
		<rdfs:comment xml:lang="OWLManchester">platform:implementsInterface some JavaUtilAPI</rdfs:comment>
	</owl:Class>
	<owl:Class rdf:about="#JavaUtilJarClassLibrary">
		<rdfs:subClassOf rdf:resource="&j2me-pp-1_0;JavaUtilJarClassLibrary"/>
		<rdfs:subClassOf rdf:resource="&j2se-1_3;JavaUtilJarClassLibrary"/>
		<rdfs:comment xml:lang="en">JavaLibrary implementing the java.util.jar package for J2ME PP 1.1</rdfs:comment>
		<rdfs:comment xml:lang="OWLManchester">platform:implementsInterface some JavaUtilJarAPI</rdfs:comment>
	</owl:Class>
	<owl:Class rdf:about="#JavaUtilZipClassLibrary">
		<rdfs:subClassOf rdf:resource="&j2me-pp-1_0;JavaUtilZipClassLibrary"/>
		<rdfs:subClassOf rdf:resource="&j2se-1_3;JavaUtilZipClassLibrary"/>
		<rdfs:comment xml:lang="en">JavaLibrary implementing the java.util.zip package for J2ME PP 1.1</rdfs:comment>
		<rdfs:comment xml:lang="OWLManchester">platform:implementsInterface some JavaUtilZipAPI</rdfs:comment>
	</owl:Class>
	<owl:Class rdf:about="#JavaMathClassLibrary">
		<owl:equivalentClass rdf:resource="&j2me-pp-1_0;JavaMathClassLibrary"/>
		<owl:equivalentClass rdf:resource="&j2se-1_3;JavaMathClassLibrary"/>
		<rdfs:subClassOf rdf:resource="&java;JavaClassLibrary"/>
		<rdfs:comment xml:lang="en">JavaLibrary implementing the java.math package for J2ME PP 1.1</rdfs:comment>
		<rdfs:comment xml:lang="OWLManchester">platform:implementsInterface some JavaMathAPI</rdfs:comment>
	</owl:Class>
	<owl:Class rdf:about="#JavaTextClassLibrary">
		<rdfs:subClassOf rdf:resource="&j2me-pp-1_0;JavaTextClassLibrary"/>
		<rdfs:subClassOf rdf:resource="&j2se-1_3;JavaTextClassLibrary"/>
		<rdfs:comment xml:lang="en">JavaLibrary implementing the java.text package for J2ME PP 1.1</rdfs:comment>
		<rdfs:comment xml:lang="OWLManchester">platform:implementsInterface some JavaTextAPI</rdfs:comment>
	</owl:Class>
	<owl:Class rdf:about="#JavaAwtClassLibrary">
		<rdfs:subClassOf rdf:resource="&j2me-pp-1_0;JavaAwtClassLibrary"/>
		<rdfs:comment xml:lang="en">JavaLibrary implementing the java.awt package for J2ME PP 1.1</rdfs:comment>
		<rdfs:comment xml:lang="OWLManchester">platform:implementsInterface some JavaAwtAPI</rdfs:comment>
	</owl:Class>
	<owl:Class rdf:about="#JavaAwtImClassLibrary">
		<rdfs:subClassOf rdf:resource="&java;JavaClassLibrary"/>
		<rdfs:comment xml:lang="en">JavaLibrary implementing the java.awt.im package for J2ME PP 1.1</rdfs:comment>
		<rdfs:comment xml:lang="OWLManchester">platform:implementsInterface some JavaAwtImAPI</rdfs:comment>
	</owl:Class>
	<owl:Class rdf:about="#JavaAwtFontClassLibrary">
		<rdfs:subClassOf rdf:resource="&java;JavaClassLibrary"/>
		<rdfs:comment xml:lang="en">JavaLibrary implementing the java.awt.font package for J2ME PP 1.1</rdfs:comment>
		<rdfs:comment xml:lang="OWLManchester">platform:implementsInterface some JavaAwtFontAPI</rdfs:comment>
	</owl:Class>
	<owl:Class rdf:about="#JavaAwtEventClassLibrary">
		<rdfs:subClassOf rdf:resource="&j2me-pp-1_0;JavaAwtEventClassLibrary"/>
		<rdfs:comment xml:lang="en">JavaLibrary implementing the java.awt.event package for J2ME PP 1.1</rdfs:comment>
		<rdfs:comment xml:lang="OWLManchester">platform:implementsInterface some JavaAwtEventAPI</rdfs:comment>
	</owl:Class>
	<owl:Class rdf:about="#JavaAwtImageClassLibrary">
		<rdfs:subClassOf rdf:resource="&j2me-pp-1_0;JavaAwtImageClassLibrary"/>
		<rdfs:comment xml:lang="en">JavaLibrary implementing the java.awt.image package for J2ME PP 1.1</rdfs:comment>
		<rdfs:comment xml:lang="OWLManchester">platform:implementsInterface some JavaAwtImageAPI</rdfs:comment>
	</owl:Class>
	<owl:Class rdf:about="#JavaAwtColorClassLibrary">
		<owl:equivalentClass rdf:resource="&j2me-pp-1_0;JavaAwtColorClassLibrary"/>
		<rdfs:subClassOf rdf:resource="&java;JavaClassLibrary"/>
		<rdfs:comment xml:lang="en">JavaLibrary implementing the java.awt.color package for J2ME PP 1.1</rdfs:comment>
		<rdfs:comment xml:lang="OWLManchester">platform:implementsInterface some JavaAwtColorAPI</rdfs:comment>
	</owl:Class>
	<owl:Class rdf:about="#JavaAwtDatatransferClassLibrary">
		<rdfs:subClassOf rdf:resource="&j2me-pp-1_0;JavaAwtDatatransferClassLibrary"/>
		<rdfs:comment xml:lang="en">JavaLibrary implementing the java.awt.datatransfer package for J2ME PP 1.1</rdfs:comment>
		<rdfs:comment xml:lang="OWLManchester">platform:implementsInterface some JavaAwtDatatransferAPI</rdfs:comment>
	</owl:Class>
	<owl:Class rdf:about="#JavaBeansClassLibrary">
		<rdfs:subClassOf rdf:resource="&j2me-pp-1_0;JavaBeansClassLibrary"/>
		<rdfs:comment xml:lang="en">JavaLibrary implementing the java.beans package for J2ME PP 1.1</rdfs:comment>
		<rdfs:comment xml:lang="OWLManchester">platform:implementsInterface some JavaBeansAPI</rdfs:comment>
	</owl:Class>
	<owl:Class rdf:about="#JavaRmiClassLibrary">
		<rdfs:subClassOf rdf:resource="&j2me-pp-1_0;JavaRmiClassLibrary"/>
		<rdfs:comment xml:lang="en">JavaLibrary implementing the java.rmi package for J2ME PP 1.1</rdfs:comment>
		<rdfs:comment xml:lang="OWLManchester">platform:implementsInterface some JavaRmiAPI</rdfs:comment>
	</owl:Class>
	<owl:Class rdf:about="#JavaRmiRegistryClassLibrary">
		<owl:equivalentClass rdf:resource="&j2me-pp-1_0;JavaRmiRegistryClassLibrary"/>
		<rdfs:subClassOf rdf:resource="&java;JavaClassLibrary"/>
		<rdfs:comment xml:lang="en">JavaLibrary implementing the java.rmi.registry package for J2ME PP 1.1</rdfs:comment>
		<rdfs:comment xml:lang="OWLManchester">platform:implementsInterface some JavaRmiRegistryAPI</rdfs:comment>
	</owl:Class>
	<owl:Class rdf:about="#JavaAppletClassLibrary">
		<rdfs:subClassOf rdf:resource="&j2me-pp-1_0;JavaAppletClassLibrary"/>
		<rdfs:comment xml:lang="en">JavaLibrary implementing the java.applet package for J2ME PP 1.1</rdfs:comment>
		<rdfs:comment xml:lang="OWLManchester">platform:implementsInterface some JavaAppletAPI</rdfs:comment>
	</owl:Class>
	<owl:Class rdf:about="#JavaxSecurityAuthX500ClassLibrary">
		<rdfs:subClassOf rdf:resource="&java;JavaClassLibrary"/>
		<rdfs:comment xml:lang="en">JavaLibrary implementing the javax.security.auth.x500 package for J2ME PP 1.1</rdfs:comment>
		<rdfs:comment xml:lang="OWLManchester">platform:implementsInterface some JavaxSecurityAuthX500API</rdfs:comment>
	</owl:Class>
	<owl:Class rdf:about="#JavaxMicroeditionIoClassLibrary">
		<rdfs:subClassOf rdf:resource="&j2me-pp-1_0;JavaxMicroeditionIoClassLibrary"/>
		<rdfs:comment xml:lang="en">JavaLibrary implementing the javax.microedition.io package for J2ME PP 1.1</rdfs:comment>
		<rdfs:comment xml:lang="OWLManchester">platform:implementsInterface some JavaxMicroeditionIoAPI</rdfs:comment>
	</owl:Class>
	<owl:Class rdf:about="#JavaxMicroeditionPkiClassLibrary">
		<rdfs:subClassOf rdf:resource="&java;JavaClassLibrary"/>
		<rdfs:comment xml:lang="en">JavaLibrary implementing the javax.microedition.pki package for J2ME PP 1.1</rdfs:comment>
		<rdfs:comment xml:lang="OWLManchester">platform:implementsInterface some JavaxMicroeditionPkiAPI</rdfs:comment>
	</owl:Class>
	<owl:Class rdf:about="#JavaxMicroeditionXletClassLibrary">
		<rdfs:subClassOf rdf:resource="&j2me-pp-1_0;JavaxMicroeditionXletClassLibrary"/>
		<rdfs:comment xml:lang="en">JavaLibrary implementing the javax.microedition.xlet package for J2ME PP 1.1</rdfs:comment>
		<rdfs:comment xml:lang="OWLManchester">platform:implementsInterface some JavaxMicroeditionXletAPI</rdfs:comment>
	</owl:Class>
	<owl:Class rdf:about="#JavaxMicroeditionXletIxcClassLibrary">
		<rdfs:subClassOf rdf:resource="&j2me-pp-1_0;JavaxMicroeditionXletIxcClassLibrary"/>
		<rdfs:comment xml:lang="en">JavaLibrary implementing the javax.microedition.xlet.ixc package for J2ME PP 1.1</rdfs:comment>
		<rdfs:comment xml:lang="OWLManchester">platform:implementsInterface some JavaxMicroeditionXletIxcAPI</rdfs:comment>
	</owl:Class>
</rdf:RDF>
