<?xml version="1.0" encoding="ISO-8859-1"?>
<!DOCTYPE rdf:RDF [
	<!ENTITY isa "http://soft.vub.ac.be/platformkit/2010/1/isa.owl#">
	<!ENTITY j2me-pp-1_0 "http://soft.vub.ac.be/platformkit/2010/1/j2me-pp-1_0.owl#">
	<!ENTITY xsd "http://www.w3.org/2001/XMLSchema#">
	<!ENTITY j2se-1_2 "http://soft.vub.ac.be/platformkit/2010/1/j2se-1_2.owl#">
	<!ENTITY java "http://soft.vub.ac.be/platformkit/2010/1/java.owl#">
	<!ENTITY platform "http://soft.vub.ac.be/platformkit/2010/1/platform.owl#">
	<!ENTITY rdf "http://www.w3.org/1999/02/22-rdf-syntax-ns#">
	<!ENTITY rdfs "http://www.w3.org/2000/01/rdf-schema#">
	<!ENTITY owl "http://www.w3.org/2002/07/owl#">
]>
<rdf:RDF
	 xmlns="http://soft.vub.ac.be/platformkit/2010/1/j2se-1_3.owl#"
	 xml:base="http://soft.vub.ac.be/platformkit/2010/1/j2se-1_3.owl"
	 xmlns:isa="&isa;"
	 xmlns:j2me-pp-1_0="&j2me-pp-1_0;"
	 xmlns:xsd="&xsd;"
	 xmlns:j2se-1_2="&j2se-1_2;"
	 xmlns:java="&java;"
	 xmlns:platform="&platform;"
	 xmlns:rdf="&rdf;"
	 xmlns:rdfs="&rdfs;"
	 xmlns:owl="&owl;"
>

	<owl:Ontology rdf:about="">
		<owl:versionInfo>$Id$</owl:versionInfo>
		<owl:imports rdf:resource="http://soft.vub.ac.be/platformkit/2010/1/platform.owl"/>
		<owl:imports rdf:resource="http://soft.vub.ac.be/platformkit/2010/1/java.owl"/>
		<owl:imports rdf:resource="http://soft.vub.ac.be/platformkit/2010/1/j2se-1_2.owl"/>
		<owl:imports rdf:resource="http://soft.vub.ac.be/platformkit/2010/1/isa.owl"/>
		<owl:imports rdf:resource="http://soft.vub.ac.be/platformkit/2010/1/j2me-pp-1_0.owl"/>
		<rdfs:comment xml:lang="en">Generated by [UML2ToSimplifiedPackageAPIOntology.atl 8080 2010-03-18 10:46:40Z dwagelaa], [UML2ToPackageAPIOntology.atl 8082 2010-03-18 21:11:00Z dwagelaa], [UML2ToAPIOntology.atl 8082 2010-03-18 21:11:00Z dwagelaa], and [UML2Comparison.atl 8082 2010-03-18 21:11:00Z dwagelaa]</rdfs:comment>
		<rdfs:comment>Dennis Wagelaar &lt;dennis.wagelaar@vub.ac.be&gt;</rdfs:comment>
		<rdfs:comment xml:lang="en">&#169; 2010, Vrije Universiteit Brussel. All rights reserved.</rdfs:comment>
		<rdfs:label xml:lang="en">J2SE 1.3</rdfs:label>
	</owl:Ontology>
	<owl:Class rdf:about="#J2SE1_3API">
		<rdfs:subClassOf rdf:resource="#JavaIoAPI"/>
		<rdfs:subClassOf rdf:resource="#JavaLangAPI"/>
		<rdfs:subClassOf rdf:resource="#JavaLangReflectAPI"/>
		<rdfs:subClassOf rdf:resource="#JavaLangRefAPI"/>
		<rdfs:subClassOf rdf:resource="#JavaNetAPI"/>
		<rdfs:subClassOf rdf:resource="#JavaSecurityAPI"/>
		<rdfs:subClassOf rdf:resource="#JavaSecurityCertAPI"/>
		<rdfs:subClassOf rdf:resource="#JavaSecuritySpecAPI"/>
		<rdfs:subClassOf rdf:resource="#JavaSecurityInterfacesAPI"/>
		<rdfs:subClassOf rdf:resource="#JavaSecurityAclAPI"/>
		<rdfs:subClassOf rdf:resource="#JavaUtilAPI"/>
		<rdfs:subClassOf rdf:resource="#JavaUtilJarAPI"/>
		<rdfs:subClassOf rdf:resource="#JavaUtilZipAPI"/>
		<rdfs:subClassOf rdf:resource="#JavaMathAPI"/>
		<rdfs:subClassOf rdf:resource="#JavaTextAPI"/>
		<rdfs:subClassOf rdf:resource="#JavaTextResourcesAPI"/>
		<rdfs:subClassOf rdf:resource="#JavaAwtAPI"/>
		<rdfs:subClassOf rdf:resource="#JavaAwtGeomAPI"/>
		<rdfs:subClassOf rdf:resource="#JavaAwtEventAPI"/>
		<rdfs:subClassOf rdf:resource="#JavaAwtFontAPI"/>
		<rdfs:subClassOf rdf:resource="#JavaAwtImageAPI"/>
		<rdfs:subClassOf rdf:resource="#JavaAwtImageRenderableAPI"/>
		<rdfs:subClassOf rdf:resource="#JavaAwtDndAPI"/>
		<rdfs:subClassOf rdf:resource="#JavaAwtImAPI"/>
		<rdfs:subClassOf rdf:resource="#JavaAwtImSpiAPI"/>
		<rdfs:subClassOf rdf:resource="#JavaAwtColorAPI"/>
		<rdfs:subClassOf rdf:resource="#JavaAwtDatatransferAPI"/>
		<rdfs:subClassOf rdf:resource="#JavaAwtPrintAPI"/>
		<rdfs:subClassOf rdf:resource="#JavaBeansAPI"/>
		<rdfs:subClassOf rdf:resource="#JavaBeansBeancontextAPI"/>
		<rdfs:subClassOf rdf:resource="#JavaAppletAPI"/>
		<rdfs:subClassOf rdf:resource="#JavaRmiAPI"/>
		<rdfs:subClassOf rdf:resource="#JavaRmiServerAPI"/>
		<rdfs:subClassOf rdf:resource="#JavaRmiDgcAPI"/>
		<rdfs:subClassOf rdf:resource="#JavaRmiRegistryAPI"/>
		<rdfs:subClassOf rdf:resource="#JavaRmiActivationAPI"/>
		<rdfs:subClassOf rdf:resource="#JavaSqlAPI"/>
		<rdfs:subClassOf rdf:resource="#JavaxAccessibilityAPI"/>
		<rdfs:subClassOf rdf:resource="#JavaxSwingAPI"/>
		<rdfs:subClassOf rdf:resource="#JavaxSwingTextAPI"/>
		<rdfs:subClassOf rdf:resource="#JavaxSwingTextHtmlAPI"/>
		<rdfs:subClassOf rdf:resource="#JavaxSwingTextHtmlParserAPI"/>
		<rdfs:subClassOf rdf:resource="#JavaxSwingTextRtfAPI"/>
		<rdfs:subClassOf rdf:resource="#JavaxSwingEventAPI"/>
		<rdfs:subClassOf rdf:resource="#JavaxSwingPlafAPI"/>
		<rdfs:subClassOf rdf:resource="#JavaxSwingPlafBasicAPI"/>
		<rdfs:subClassOf rdf:resource="#JavaxSwingPlafMetalAPI"/>
		<rdfs:subClassOf rdf:resource="#JavaxSwingPlafMultiAPI"/>
		<rdfs:subClassOf rdf:resource="#JavaxSwingUndoAPI"/>
		<rdfs:subClassOf rdf:resource="#JavaxSwingTreeAPI"/>
		<rdfs:subClassOf rdf:resource="#JavaxSwingTableAPI"/>
		<rdfs:subClassOf rdf:resource="#JavaxSwingBorderAPI"/>
		<rdfs:subClassOf rdf:resource="#JavaxSwingColorchooserAPI"/>
		<rdfs:subClassOf rdf:resource="#JavaxSwingFilechooserAPI"/>
		<rdfs:subClassOf rdf:resource="#JavaxNamingAPI"/>
		<rdfs:subClassOf rdf:resource="#JavaxNamingDirectoryAPI"/>
		<rdfs:subClassOf rdf:resource="#JavaxNamingEventAPI"/>
		<rdfs:subClassOf rdf:resource="#JavaxNamingLdapAPI"/>
		<rdfs:subClassOf rdf:resource="#JavaxNamingSpiAPI"/>
		<rdfs:subClassOf rdf:resource="#JavaxSoundMidiAPI"/>
		<rdfs:subClassOf rdf:resource="#JavaxSoundMidiSpiAPI"/>
		<rdfs:subClassOf rdf:resource="#JavaxSoundSampledAPI"/>
		<rdfs:subClassOf rdf:resource="#JavaxSoundSampledSpiAPI"/>
		<rdfs:subClassOf rdf:resource="#JavaxRmiAPI"/>
		<rdfs:subClassOf rdf:resource="#JavaxRmiCORBAAPI"/>
		<rdfs:subClassOf rdf:resource="#JavaxTransactionAPI"/>
		<rdfs:subClassOf rdf:resource="#OrgOmgCORBA_2_3API"/>
		<rdfs:subClassOf rdf:resource="#OrgOmgCORBA_2_3PortableAPI"/>
		<rdfs:subClassOf rdf:resource="#OrgOmgCORBAAPI"/>
		<rdfs:subClassOf rdf:resource="#OrgOmgCORBAPortableAPI"/>
		<rdfs:subClassOf rdf:resource="#OrgOmgCORBATypeCodePackageAPI"/>
		<rdfs:subClassOf rdf:resource="#OrgOmgCORBAORBPackageAPI"/>
		<rdfs:subClassOf rdf:resource="#OrgOmgCORBADynAnyPackageAPI"/>
		<rdfs:subClassOf rdf:resource="#OrgOmgSendingContextAPI"/>
		<rdfs:subClassOf rdf:resource="#OrgOmgCosNamingAPI"/>
		<rdfs:subClassOf rdf:resource="#OrgOmgCosNamingNamingContextPackageAPI"/>
		<rdfs:subClassOf rdf:resource="#OrgOmgStubJavaRmiAPI"/>
		<rdfs:comment xml:lang="en">J2SE 1.3 API</rdfs:comment>
		<rdfs:comment xml:lang="OWLManchester">platform:comprisesInterfacePart some JavaIo and platform:comprisesInterfacePart some JavaLang and platform:comprisesInterfacePart some JavaLangReflect and platform:comprisesInterfacePart some JavaLangRef and platform:comprisesInterfacePart some JavaNet and platform:comprisesInterfacePart some JavaSecurity and platform:comprisesInterfacePart some JavaSecurityCert and platform:comprisesInterfacePart some JavaSecuritySpec and platform:comprisesInterfacePart some JavaSecurityInterfaces and platform:comprisesInterfacePart some JavaSecurityAcl and platform:comprisesInterfacePart some JavaUtil and platform:comprisesInterfacePart some JavaUtilJar and platform:comprisesInterfacePart some JavaUtilZip and platform:comprisesInterfacePart some JavaMath and platform:comprisesInterfacePart some JavaText and platform:comprisesInterfacePart some JavaTextResources and platform:comprisesInterfacePart some JavaAwt and platform:comprisesInterfacePart some JavaAwtGeom and platform:comprisesInterfacePart some JavaAwtEvent and platform:comprisesInterfacePart some JavaAwtFont and platform:comprisesInterfacePart some JavaAwtImage and platform:comprisesInterfacePart some JavaAwtImageRenderable and platform:comprisesInterfacePart some JavaAwtDnd and platform:comprisesInterfacePart some JavaAwtIm and platform:comprisesInterfacePart some JavaAwtImSpi and platform:comprisesInterfacePart some JavaAwtColor and platform:comprisesInterfacePart some JavaAwtDatatransfer and platform:comprisesInterfacePart some JavaAwtPrint and platform:comprisesInterfacePart some JavaBeans and platform:comprisesInterfacePart some JavaBeansBeancontext and platform:comprisesInterfacePart some JavaApplet and platform:comprisesInterfacePart some JavaRmi and platform:comprisesInterfacePart some JavaRmiServer and platform:comprisesInterfacePart some JavaRmiDgc and platform:comprisesInterfacePart some JavaRmiRegistry and platform:comprisesInterfacePart some JavaRmiActivation and platform:comprisesInterfacePart some JavaSql and platform:comprisesInterfacePart some JavaxAccessibility and platform:comprisesInterfacePart some JavaxSwing and platform:comprisesInterfacePart some JavaxSwingText and platform:comprisesInterfacePart some JavaxSwingTextHtml and platform:comprisesInterfacePart some JavaxSwingTextHtmlParser and platform:comprisesInterfacePart some JavaxSwingTextRtf and platform:comprisesInterfacePart some JavaxSwingEvent and platform:comprisesInterfacePart some JavaxSwingPlaf and platform:comprisesInterfacePart some JavaxSwingPlafBasic and platform:comprisesInterfacePart some JavaxSwingPlafMetal and platform:comprisesInterfacePart some JavaxSwingPlafMulti and platform:comprisesInterfacePart some JavaxSwingUndo and platform:comprisesInterfacePart some JavaxSwingTree and platform:comprisesInterfacePart some JavaxSwingTable and platform:comprisesInterfacePart some JavaxSwingBorder and platform:comprisesInterfacePart some JavaxSwingColorchooser and platform:comprisesInterfacePart some JavaxSwingFilechooser and platform:comprisesInterfacePart some JavaxNaming and platform:comprisesInterfacePart some JavaxNamingDirectory and platform:comprisesInterfacePart some JavaxNamingEvent and platform:comprisesInterfacePart some JavaxNamingLdap and platform:comprisesInterfacePart some JavaxNamingSpi and platform:comprisesInterfacePart some JavaxSoundMidi and platform:comprisesInterfacePart some JavaxSoundMidiSpi and platform:comprisesInterfacePart some JavaxSoundSampled and platform:comprisesInterfacePart some JavaxSoundSampledSpi and platform:comprisesInterfacePart some JavaxRmi and platform:comprisesInterfacePart some JavaxRmiCORBA and platform:comprisesInterfacePart some JavaxTransaction and platform:comprisesInterfacePart some OrgOmgCORBA_2_3 and platform:comprisesInterfacePart some OrgOmgCORBA_2_3Portable and platform:comprisesInterfacePart some OrgOmgCORBA and platform:comprisesInterfacePart some OrgOmgCORBAPortable and platform:comprisesInterfacePart some OrgOmgCORBATypeCodePackage and platform:comprisesInterfacePart some OrgOmgCORBAORBPackage and platform:comprisesInterfacePart some OrgOmgCORBADynAnyPackage and platform:comprisesInterfacePart some OrgOmgSendingContext and platform:comprisesInterfacePart some OrgOmgCosNaming and platform:comprisesInterfacePart some OrgOmgCosNamingNamingContextPackage and platform:comprisesInterfacePart some OrgOmgStubJavaRmi</rdfs:comment>
	</owl:Class>
	<owl:Class rdf:about="#J2SE1_3ClassLibrary">
		<rdfs:subClassOf rdf:resource="#JavaIoClassLibrary"/>
		<rdfs:subClassOf rdf:resource="#JavaLangClassLibrary"/>
		<rdfs:subClassOf rdf:resource="#JavaLangReflectClassLibrary"/>
		<rdfs:subClassOf rdf:resource="#JavaLangRefClassLibrary"/>
		<rdfs:subClassOf rdf:resource="#JavaNetClassLibrary"/>
		<rdfs:subClassOf rdf:resource="#JavaSecurityClassLibrary"/>
		<rdfs:subClassOf rdf:resource="#JavaSecurityCertClassLibrary"/>
		<rdfs:subClassOf rdf:resource="#JavaSecuritySpecClassLibrary"/>
		<rdfs:subClassOf rdf:resource="#JavaSecurityInterfacesClassLibrary"/>
		<rdfs:subClassOf rdf:resource="#JavaSecurityAclClassLibrary"/>
		<rdfs:subClassOf rdf:resource="#JavaUtilClassLibrary"/>
		<rdfs:subClassOf rdf:resource="#JavaUtilJarClassLibrary"/>
		<rdfs:subClassOf rdf:resource="#JavaUtilZipClassLibrary"/>
		<rdfs:subClassOf rdf:resource="#JavaMathClassLibrary"/>
		<rdfs:subClassOf rdf:resource="#JavaTextClassLibrary"/>
		<rdfs:subClassOf rdf:resource="#JavaTextResourcesClassLibrary"/>
		<rdfs:subClassOf rdf:resource="#JavaAwtClassLibrary"/>
		<rdfs:subClassOf rdf:resource="#JavaAwtGeomClassLibrary"/>
		<rdfs:subClassOf rdf:resource="#JavaAwtEventClassLibrary"/>
		<rdfs:subClassOf rdf:resource="#JavaAwtFontClassLibrary"/>
		<rdfs:subClassOf rdf:resource="#JavaAwtImageClassLibrary"/>
		<rdfs:subClassOf rdf:resource="#JavaAwtImageRenderableClassLibrary"/>
		<rdfs:subClassOf rdf:resource="#JavaAwtDndClassLibrary"/>
		<rdfs:subClassOf rdf:resource="#JavaAwtImClassLibrary"/>
		<rdfs:subClassOf rdf:resource="#JavaAwtImSpiClassLibrary"/>
		<rdfs:subClassOf rdf:resource="#JavaAwtColorClassLibrary"/>
		<rdfs:subClassOf rdf:resource="#JavaAwtDatatransferClassLibrary"/>
		<rdfs:subClassOf rdf:resource="#JavaAwtPrintClassLibrary"/>
		<rdfs:subClassOf rdf:resource="#JavaBeansClassLibrary"/>
		<rdfs:subClassOf rdf:resource="#JavaBeansBeancontextClassLibrary"/>
		<rdfs:subClassOf rdf:resource="#JavaAppletClassLibrary"/>
		<rdfs:subClassOf rdf:resource="#JavaRmiClassLibrary"/>
		<rdfs:subClassOf rdf:resource="#JavaRmiServerClassLibrary"/>
		<rdfs:subClassOf rdf:resource="#JavaRmiDgcClassLibrary"/>
		<rdfs:subClassOf rdf:resource="#JavaRmiRegistryClassLibrary"/>
		<rdfs:subClassOf rdf:resource="#JavaRmiActivationClassLibrary"/>
		<rdfs:subClassOf rdf:resource="#JavaSqlClassLibrary"/>
		<rdfs:subClassOf rdf:resource="#JavaxAccessibilityClassLibrary"/>
		<rdfs:subClassOf rdf:resource="#JavaxSwingClassLibrary"/>
		<rdfs:subClassOf rdf:resource="#JavaxSwingTextClassLibrary"/>
		<rdfs:subClassOf rdf:resource="#JavaxSwingTextHtmlClassLibrary"/>
		<rdfs:subClassOf rdf:resource="#JavaxSwingTextHtmlParserClassLibrary"/>
		<rdfs:subClassOf rdf:resource="#JavaxSwingTextRtfClassLibrary"/>
		<rdfs:subClassOf rdf:resource="#JavaxSwingEventClassLibrary"/>
		<rdfs:subClassOf rdf:resource="#JavaxSwingPlafClassLibrary"/>
		<rdfs:subClassOf rdf:resource="#JavaxSwingPlafBasicClassLibrary"/>
		<rdfs:subClassOf rdf:resource="#JavaxSwingPlafMetalClassLibrary"/>
		<rdfs:subClassOf rdf:resource="#JavaxSwingPlafMultiClassLibrary"/>
		<rdfs:subClassOf rdf:resource="#JavaxSwingUndoClassLibrary"/>
		<rdfs:subClassOf rdf:resource="#JavaxSwingTreeClassLibrary"/>
		<rdfs:subClassOf rdf:resource="#JavaxSwingTableClassLibrary"/>
		<rdfs:subClassOf rdf:resource="#JavaxSwingBorderClassLibrary"/>
		<rdfs:subClassOf rdf:resource="#JavaxSwingColorchooserClassLibrary"/>
		<rdfs:subClassOf rdf:resource="#JavaxSwingFilechooserClassLibrary"/>
		<rdfs:subClassOf rdf:resource="#JavaxNamingClassLibrary"/>
		<rdfs:subClassOf rdf:resource="#JavaxNamingDirectoryClassLibrary"/>
		<rdfs:subClassOf rdf:resource="#JavaxNamingEventClassLibrary"/>
		<rdfs:subClassOf rdf:resource="#JavaxNamingLdapClassLibrary"/>
		<rdfs:subClassOf rdf:resource="#JavaxNamingSpiClassLibrary"/>
		<rdfs:subClassOf rdf:resource="#JavaxSoundMidiClassLibrary"/>
		<rdfs:subClassOf rdf:resource="#JavaxSoundMidiSpiClassLibrary"/>
		<rdfs:subClassOf rdf:resource="#JavaxSoundSampledClassLibrary"/>
		<rdfs:subClassOf rdf:resource="#JavaxSoundSampledSpiClassLibrary"/>
		<rdfs:subClassOf rdf:resource="#JavaxRmiClassLibrary"/>
		<rdfs:subClassOf rdf:resource="#JavaxRmiCORBAClassLibrary"/>
		<rdfs:subClassOf rdf:resource="#JavaxTransactionClassLibrary"/>
		<rdfs:subClassOf rdf:resource="#OrgOmgCORBA_2_3ClassLibrary"/>
		<rdfs:subClassOf rdf:resource="#OrgOmgCORBA_2_3PortableClassLibrary"/>
		<rdfs:subClassOf rdf:resource="#OrgOmgCORBAClassLibrary"/>
		<rdfs:subClassOf rdf:resource="#OrgOmgCORBAPortableClassLibrary"/>
		<rdfs:subClassOf rdf:resource="#OrgOmgCORBATypeCodePackageClassLibrary"/>
		<rdfs:subClassOf rdf:resource="#OrgOmgCORBAORBPackageClassLibrary"/>
		<rdfs:subClassOf rdf:resource="#OrgOmgCORBADynAnyPackageClassLibrary"/>
		<rdfs:subClassOf rdf:resource="#OrgOmgSendingContextClassLibrary"/>
		<rdfs:subClassOf rdf:resource="#OrgOmgCosNamingClassLibrary"/>
		<rdfs:subClassOf rdf:resource="#OrgOmgCosNamingNamingContextPackageClassLibrary"/>
		<rdfs:subClassOf rdf:resource="#OrgOmgStubJavaRmiClassLibrary"/>
		<rdfs:comment xml:lang="en">Java class library implementing the J2SE 1.3 API</rdfs:comment>
		<rdfs:comment xml:lang="OWLManchester">platform:implementsInterface some J2SE1_3API</rdfs:comment>
	</owl:Class>
	<owl:Class rdf:about="#J2SE1_3BytecodeFormat">
		<owl:equivalentClass rdf:resource="&j2me-pp-1_0;J2MEPP1_0BytecodeFormat"/>
		<rdfs:subClassOf rdf:resource="&j2se-1_2;J2SE1_2BytecodeFormat"/>
		<rdfs:comment xml:lang="en">J2SE 1.3 bytecode format</rdfs:comment>
		<rdfs:comment xml:lang="OWLManchester">java:majorVersionNumber some xsd:integer[>="47"^^xsd:integer] and java:preverified value false</rdfs:comment>
	</owl:Class>
	<J2SE1_3BytecodeFormat rdf:about="#theJ2SE1_3BytecodeFormat">
		<java:preverified rdf:datatype="http://www.w3.org/2001/XMLSchema#boolean">false</java:preverified>
		<java:minorVersionNumber rdf:datatype="http://www.w3.org/2001/XMLSchema#integer">0</java:minorVersionNumber>
		<java:majorVersionNumber rdf:datatype="http://www.w3.org/2001/XMLSchema#integer">47</java:majorVersionNumber>
	</J2SE1_3BytecodeFormat>
	<J2SE1_3API rdf:about="#theJ2SE1_3API">
		<platform:comprisesInterfacePart rdf:resource="#theOrgOmgStubJavaRmiPart"/>
		<platform:comprisesInterfacePart rdf:resource="#theOrgOmgCosNamingNamingContextPackagePart"/>
		<platform:comprisesInterfacePart rdf:resource="#theOrgOmgCosNamingPart"/>
		<platform:comprisesInterfacePart rdf:resource="#theOrgOmgSendingContextPart"/>
		<platform:comprisesInterfacePart rdf:resource="#theOrgOmgCORBADynAnyPackagePart"/>
		<platform:comprisesInterfacePart rdf:resource="#theOrgOmgCORBAORBPackagePart"/>
		<platform:comprisesInterfacePart rdf:resource="#theOrgOmgCORBATypeCodePackagePart"/>
		<platform:comprisesInterfacePart rdf:resource="#theOrgOmgCORBAPortablePart"/>
		<platform:comprisesInterfacePart rdf:resource="#theOrgOmgCORBAPart"/>
		<platform:comprisesInterfacePart rdf:resource="#theOrgOmgCORBA_2_3PortablePart"/>
		<platform:comprisesInterfacePart rdf:resource="#theOrgOmgCORBA_2_3Part"/>
		<platform:comprisesInterfacePart rdf:resource="#theJavaxTransactionPart"/>
		<platform:comprisesInterfacePart rdf:resource="#theJavaxRmiCORBAPart"/>
		<platform:comprisesInterfacePart rdf:resource="#theJavaxRmiPart"/>
		<platform:comprisesInterfacePart rdf:resource="#theJavaxSoundSampledSpiPart"/>
		<platform:comprisesInterfacePart rdf:resource="#theJavaxSoundSampledPart"/>
		<platform:comprisesInterfacePart rdf:resource="#theJavaxSoundMidiSpiPart"/>
		<platform:comprisesInterfacePart rdf:resource="#theJavaxSoundMidiPart"/>
		<platform:comprisesInterfacePart rdf:resource="#theJavaxNamingSpiPart"/>
		<platform:comprisesInterfacePart rdf:resource="#theJavaxNamingLdapPart"/>
		<platform:comprisesInterfacePart rdf:resource="#theJavaxNamingEventPart"/>
		<platform:comprisesInterfacePart rdf:resource="#theJavaxNamingDirectoryPart"/>
		<platform:comprisesInterfacePart rdf:resource="#theJavaxNamingPart"/>
		<platform:comprisesInterfacePart rdf:resource="#theJavaxSwingFilechooserPart"/>
		<platform:comprisesInterfacePart rdf:resource="#theJavaxSwingColorchooserPart"/>
		<platform:comprisesInterfacePart rdf:resource="#theJavaxSwingBorderPart"/>
		<platform:comprisesInterfacePart rdf:resource="#theJavaxSwingTablePart"/>
		<platform:comprisesInterfacePart rdf:resource="#theJavaxSwingTreePart"/>
		<platform:comprisesInterfacePart rdf:resource="#theJavaxSwingUndoPart"/>
		<platform:comprisesInterfacePart rdf:resource="#theJavaxSwingPlafMultiPart"/>
		<platform:comprisesInterfacePart rdf:resource="#theJavaxSwingPlafMetalPart"/>
		<platform:comprisesInterfacePart rdf:resource="#theJavaxSwingPlafBasicPart"/>
		<platform:comprisesInterfacePart rdf:resource="#theJavaxSwingPlafPart"/>
		<platform:comprisesInterfacePart rdf:resource="#theJavaxSwingEventPart"/>
		<platform:comprisesInterfacePart rdf:resource="#theJavaxSwingTextRtfPart"/>
		<platform:comprisesInterfacePart rdf:resource="#theJavaxSwingTextHtmlParserPart"/>
		<platform:comprisesInterfacePart rdf:resource="#theJavaxSwingTextHtmlPart"/>
		<platform:comprisesInterfacePart rdf:resource="#theJavaxSwingTextPart"/>
		<platform:comprisesInterfacePart rdf:resource="#theJavaxSwingPart"/>
		<platform:comprisesInterfacePart rdf:resource="#theJavaxAccessibilityPart"/>
		<platform:comprisesInterfacePart rdf:resource="#theJavaSqlPart"/>
		<platform:comprisesInterfacePart rdf:resource="#theJavaRmiActivationPart"/>
		<platform:comprisesInterfacePart rdf:resource="#theJavaRmiRegistryPart"/>
		<platform:comprisesInterfacePart rdf:resource="#theJavaRmiDgcPart"/>
		<platform:comprisesInterfacePart rdf:resource="#theJavaRmiServerPart"/>
		<platform:comprisesInterfacePart rdf:resource="#theJavaRmiPart"/>
		<platform:comprisesInterfacePart rdf:resource="#theJavaAppletPart"/>
		<platform:comprisesInterfacePart rdf:resource="#theJavaBeansBeancontextPart"/>
		<platform:comprisesInterfacePart rdf:resource="#theJavaBeansPart"/>
		<platform:comprisesInterfacePart rdf:resource="#theJavaAwtPrintPart"/>
		<platform:comprisesInterfacePart rdf:resource="#theJavaAwtDatatransferPart"/>
		<platform:comprisesInterfacePart rdf:resource="#theJavaAwtColorPart"/>
		<platform:comprisesInterfacePart rdf:resource="#theJavaAwtImSpiPart"/>
		<platform:comprisesInterfacePart rdf:resource="#theJavaAwtImPart"/>
		<platform:comprisesInterfacePart rdf:resource="#theJavaAwtDndPart"/>
		<platform:comprisesInterfacePart rdf:resource="#theJavaAwtImageRenderablePart"/>
		<platform:comprisesInterfacePart rdf:resource="#theJavaAwtImagePart"/>
		<platform:comprisesInterfacePart rdf:resource="#theJavaAwtFontPart"/>
		<platform:comprisesInterfacePart rdf:resource="#theJavaAwtEventPart"/>
		<platform:comprisesInterfacePart rdf:resource="#theJavaAwtGeomPart"/>
		<platform:comprisesInterfacePart rdf:resource="#theJavaAwtPart"/>
		<platform:comprisesInterfacePart rdf:resource="#theJavaTextResourcesPart"/>
		<platform:comprisesInterfacePart rdf:resource="#theJavaTextPart"/>
		<platform:comprisesInterfacePart rdf:resource="#theJavaMathPart"/>
		<platform:comprisesInterfacePart rdf:resource="#theJavaUtilZipPart"/>
		<platform:comprisesInterfacePart rdf:resource="#theJavaUtilJarPart"/>
		<platform:comprisesInterfacePart rdf:resource="#theJavaUtilPart"/>
		<platform:comprisesInterfacePart rdf:resource="#theJavaSecurityAclPart"/>
		<platform:comprisesInterfacePart rdf:resource="#theJavaSecurityInterfacesPart"/>
		<platform:comprisesInterfacePart rdf:resource="#theJavaSecuritySpecPart"/>
		<platform:comprisesInterfacePart rdf:resource="#theJavaSecurityCertPart"/>
		<platform:comprisesInterfacePart rdf:resource="#theJavaSecurityPart"/>
		<platform:comprisesInterfacePart rdf:resource="#theJavaNetPart"/>
		<platform:comprisesInterfacePart rdf:resource="#theJavaLangRefPart"/>
		<platform:comprisesInterfacePart rdf:resource="#theJavaLangReflectPart"/>
		<platform:comprisesInterfacePart rdf:resource="#theJavaLangPart"/>
		<platform:comprisesInterfacePart rdf:resource="#theJavaIoPart"/>
	</J2SE1_3API>
	<owl:Class rdf:about="#J2SE1_3VM">
		<owl:equivalentClass>
			<owl:Restriction>
				<owl:onProperty rdf:resource="&platform;implementsInterface"/>
				<owl:someValuesFrom rdf:resource="#J2SE1_3BytecodeFormat"/>
			</owl:Restriction>
		</owl:equivalentClass>
		<rdfs:subClassOf rdf:resource="&java;JavaVM"/>
		<rdfs:comment xml:lang="en">J2SE 1.3 virtual machine</rdfs:comment>
	</owl:Class>
	<owl:Class rdf:about="#J2SE1_3JRE">
		<owl:equivalentClass>
			<owl:Class >
				<owl:intersectionOf rdf:parseType="Collection">
					<owl:Restriction>
						<owl:onProperty rdf:resource="&platform;providesFeature"/>
						<owl:someValuesFrom rdf:resource="#J2SE1_3ClassLibrary"/>
					</owl:Restriction>
					<owl:Restriction>
						<owl:onProperty rdf:resource="&platform;providesFeature"/>
						<owl:someValuesFrom rdf:resource="#J2SE1_3VM"/>
					</owl:Restriction>
				</owl:intersectionOf>
			</owl:Class>
		</owl:equivalentClass>
		<rdfs:subClassOf rdf:resource="&java;JRE"/>
		<rdfs:comment xml:lang="en">J2SE 1.3 Java Runtime Environment</rdfs:comment>
	</owl:Class>
	<owl:Class rdf:about="#JavaIo">
		<rdfs:subClassOf rdf:resource="&j2me-pp-1_0;JavaIo"/>
		<rdfs:subClassOf rdf:resource="&j2se-1_2;JavaIo"/>
		<rdfs:seeAlso rdf:resource="#JavaUtil"/>
		<rdfs:seeAlso rdf:resource="#JavaNet"/>
		<rdfs:seeAlso rdf:resource="#JavaLang"/>
		<rdfs:seeAlso rdf:resource="#JavaSecurity"/>
		<rdfs:comment xml:lang="en">Java API part implementing the java.io package for J2SE 1.3</rdfs:comment>
	</owl:Class>
	<owl:Class rdf:about="#JavaLang">
		<rdfs:subClassOf rdf:resource="&j2me-pp-1_0;JavaLang"/>
		<rdfs:subClassOf rdf:resource="&j2se-1_2;JavaLang"/>
		<rdfs:seeAlso rdf:resource="#JavaLangReflect"/>
		<rdfs:seeAlso rdf:resource="#JavaIo"/>
		<rdfs:seeAlso rdf:resource="#JavaSecurity"/>
		<rdfs:seeAlso rdf:resource="#JavaUtil"/>
		<rdfs:seeAlso rdf:resource="#JavaNet"/>
		<rdfs:comment xml:lang="en">Java API part implementing the java.lang package for J2SE 1.3</rdfs:comment>
	</owl:Class>
	<owl:Class rdf:about="#JavaLangReflect">
		<owl:equivalentClass rdf:resource="&j2me-pp-1_0;JavaLangReflect"/>
		<rdfs:subClassOf rdf:resource="&j2se-1_2;JavaLangReflect"/>
		<rdfs:seeAlso rdf:resource="#JavaLang"/>
		<rdfs:seeAlso rdf:resource="#JavaIo"/>
		<rdfs:seeAlso rdf:resource="#JavaSecurity"/>
		<rdfs:comment xml:lang="en">Java API part implementing the java.lang.reflect package for J2SE 1.3</rdfs:comment>
	</owl:Class>
	<owl:Class rdf:about="#JavaLangRef">
		<owl:equivalentClass rdf:resource="&j2me-pp-1_0;JavaLangRef"/>
		<owl:equivalentClass rdf:resource="&j2se-1_2;JavaLangRef"/>
		<rdfs:subClassOf rdf:resource="&java;JavaAPIPart"/>
		<rdfs:seeAlso rdf:resource="#JavaLang"/>
		<rdfs:comment xml:lang="en">Java API part implementing the java.lang.ref package for J2SE 1.3</rdfs:comment>
	</owl:Class>
	<owl:Class rdf:about="#JavaNet">
		<rdfs:subClassOf rdf:resource="&j2me-pp-1_0;JavaNet"/>
		<rdfs:subClassOf rdf:resource="&j2se-1_2;JavaNet"/>
		<rdfs:seeAlso rdf:resource="#JavaUtilJar"/>
		<rdfs:seeAlso rdf:resource="#JavaIo"/>
		<rdfs:seeAlso rdf:resource="#JavaSecurity"/>
		<rdfs:seeAlso rdf:resource="#JavaUtil"/>
		<rdfs:seeAlso rdf:resource="#JavaLang"/>
		<rdfs:comment xml:lang="en">Java API part implementing the java.net package for J2SE 1.3</rdfs:comment>
	</owl:Class>
	<owl:Class rdf:about="#JavaSecurity">
		<rdfs:subClassOf rdf:resource="&j2me-pp-1_0;JavaSecurity"/>
		<rdfs:subClassOf rdf:resource="&j2se-1_2;JavaSecurity"/>
		<rdfs:seeAlso rdf:resource="#JavaSecuritySpec"/>
		<rdfs:seeAlso rdf:resource="#JavaIo"/>
		<rdfs:seeAlso rdf:resource="#JavaSecurityCert"/>
		<rdfs:seeAlso rdf:resource="#JavaUtil"/>
		<rdfs:seeAlso rdf:resource="#JavaNet"/>
		<rdfs:seeAlso rdf:resource="#JavaLang"/>
		<rdfs:comment xml:lang="en">Java API part implementing the java.security package for J2SE 1.3</rdfs:comment>
	</owl:Class>
	<owl:Class rdf:about="#JavaSecurityCert">
		<owl:equivalentClass rdf:resource="&j2me-pp-1_0;JavaSecurityCert"/>
		<rdfs:subClassOf rdf:resource="&j2se-1_2;JavaSecurityCert"/>
		<rdfs:seeAlso rdf:resource="#JavaIo"/>
		<rdfs:seeAlso rdf:resource="#JavaSecurity"/>
		<rdfs:seeAlso rdf:resource="#JavaMath"/>
		<rdfs:seeAlso rdf:resource="#JavaUtil"/>
		<rdfs:seeAlso rdf:resource="#JavaLang"/>
		<rdfs:comment xml:lang="en">Java API part implementing the java.security.cert package for J2SE 1.3</rdfs:comment>
	</owl:Class>
	<owl:Class rdf:about="#JavaSecuritySpec">
		<owl:equivalentClass rdf:resource="&j2me-pp-1_0;JavaSecuritySpec"/>
		<rdfs:subClassOf rdf:resource="&j2se-1_2;JavaSecuritySpec"/>
		<rdfs:seeAlso rdf:resource="#JavaMath"/>
		<rdfs:seeAlso rdf:resource="#JavaLang"/>
		<rdfs:seeAlso rdf:resource="#JavaSecurity"/>
		<rdfs:seeAlso rdf:resource="#JavaSecurityInterfaces"/>
		<rdfs:comment xml:lang="en">Java API part implementing the java.security.spec package for J2SE 1.3</rdfs:comment>
	</owl:Class>
	<owl:Class rdf:about="#JavaSecurityInterfaces">
		<owl:equivalentClass rdf:resource="&j2me-pp-1_0;JavaSecurityInterfaces"/>
		<rdfs:subClassOf rdf:resource="&j2se-1_2;JavaSecurityInterfaces"/>
		<rdfs:seeAlso rdf:resource="#JavaMath"/>
		<rdfs:seeAlso rdf:resource="#JavaSecurity"/>
		<rdfs:comment xml:lang="en">Java API part implementing the java.security.interfaces package for J2SE 1.3</rdfs:comment>
	</owl:Class>
	<owl:Class rdf:about="#JavaSecurityAcl">
		<owl:equivalentClass rdf:resource="&j2me-pp-1_0;JavaSecurityAcl"/>
		<owl:equivalentClass rdf:resource="&j2se-1_2;JavaSecurityAcl"/>
		<rdfs:subClassOf rdf:resource="&java;JavaAPIPart"/>
		<rdfs:seeAlso rdf:resource="#JavaUtil"/>
		<rdfs:seeAlso rdf:resource="#JavaLang"/>
		<rdfs:seeAlso rdf:resource="#JavaSecurity"/>
		<rdfs:comment xml:lang="en">Java API part implementing the java.security.acl package for J2SE 1.3</rdfs:comment>
	</owl:Class>
	<owl:Class rdf:about="#JavaUtil">
		<rdfs:subClassOf rdf:resource="&j2me-pp-1_0;JavaUtil"/>
		<rdfs:subClassOf rdf:resource="&j2se-1_2;JavaUtil"/>
		<rdfs:seeAlso rdf:resource="#JavaIo"/>
		<rdfs:seeAlso rdf:resource="#JavaSecurity"/>
		<rdfs:seeAlso rdf:resource="#JavaLang"/>
		<rdfs:comment xml:lang="en">Java API part implementing the java.util package for J2SE 1.3</rdfs:comment>
	</owl:Class>
	<owl:Class rdf:about="#JavaUtilJar">
		<owl:equivalentClass rdf:resource="&j2me-pp-1_0;JavaUtilJar"/>
		<rdfs:subClassOf rdf:resource="&j2se-1_2;JavaUtilJar"/>
		<rdfs:seeAlso rdf:resource="#JavaIo"/>
		<rdfs:seeAlso rdf:resource="#JavaUtilZip"/>
		<rdfs:seeAlso rdf:resource="#JavaUtil"/>
		<rdfs:seeAlso rdf:resource="#JavaLang"/>
		<rdfs:comment xml:lang="en">Java API part implementing the java.util.jar package for J2SE 1.3</rdfs:comment>
	</owl:Class>
	<owl:Class rdf:about="#JavaUtilZip">
		<owl:equivalentClass rdf:resource="&j2me-pp-1_0;JavaUtilZip"/>
		<rdfs:subClassOf rdf:resource="&j2se-1_2;JavaUtilZip"/>
		<rdfs:seeAlso rdf:resource="#JavaUtil"/>
		<rdfs:seeAlso rdf:resource="#JavaLang"/>
		<rdfs:seeAlso rdf:resource="#JavaIo"/>
		<rdfs:comment xml:lang="en">Java API part implementing the java.util.zip package for J2SE 1.3</rdfs:comment>
	</owl:Class>
	<owl:Class rdf:about="#JavaMath">
		<owl:equivalentClass rdf:resource="&j2me-pp-1_0;JavaMath"/>
		<owl:equivalentClass rdf:resource="&j2se-1_2;JavaMath"/>
		<rdfs:subClassOf rdf:resource="&java;JavaAPIPart"/>
		<rdfs:seeAlso rdf:resource="#JavaUtil"/>
		<rdfs:seeAlso rdf:resource="#JavaLang"/>
		<rdfs:comment xml:lang="en">Java API part implementing the java.math package for J2SE 1.3</rdfs:comment>
	</owl:Class>
	<owl:Class rdf:about="#JavaText">
		<owl:equivalentClass rdf:resource="&j2me-pp-1_0;JavaText"/>
		<rdfs:subClassOf rdf:resource="&java;JavaAPIPart"/>
		<rdfs:seeAlso rdf:resource="#JavaIo"/>
		<rdfs:seeAlso rdf:resource="#JavaUtil"/>
		<rdfs:seeAlso rdf:resource="#JavaLang"/>
		<rdfs:comment xml:lang="en">Java API part implementing the java.text package for J2SE 1.3</rdfs:comment>
	</owl:Class>
	<owl:Class rdf:about="#JavaTextResources">
		<owl:equivalentClass rdf:resource="&j2me-pp-1_0;JavaTextResources"/>
		<rdfs:subClassOf rdf:resource="&java;JavaAPIPart"/>
		<rdfs:seeAlso rdf:resource="#JavaUtil"/>
		<rdfs:seeAlso rdf:resource="#JavaLang"/>
		<rdfs:comment xml:lang="en">Java API part implementing the java.text.resources package for J2SE 1.3</rdfs:comment>
	</owl:Class>
	<owl:Class rdf:about="#JavaAwt">
		<rdfs:subClassOf rdf:resource="&j2me-pp-1_0;JavaAwt"/>
		<rdfs:subClassOf rdf:resource="&j2se-1_2;JavaAwt"/>
		<rdfs:seeAlso rdf:resource="#JavaBeans"/>
		<rdfs:seeAlso rdf:resource="#JavaAwtImageRenderable"/>
		<rdfs:seeAlso rdf:resource="#JavaIo"/>
		<rdfs:seeAlso rdf:resource="#JavaAwtEvent"/>
		<rdfs:seeAlso rdf:resource="#JavaxSwingText"/>
		<rdfs:seeAlso rdf:resource="#JavaUtil"/>
		<rdfs:seeAlso rdf:resource="#JavaNet"/>
		<rdfs:seeAlso rdf:resource="#JavaAwtColor"/>
		<rdfs:seeAlso rdf:resource="#JavaAwtIm"/>
		<rdfs:seeAlso rdf:resource="#JavaAwtDnd"/>
		<rdfs:seeAlso rdf:resource="#JavaAwtDatatransfer"/>
		<rdfs:seeAlso rdf:resource="#JavaSecurity"/>
		<rdfs:seeAlso rdf:resource="#JavaAwtImage"/>
		<rdfs:seeAlso rdf:resource="#JavaAwtGeom"/>
		<rdfs:seeAlso rdf:resource="#JavaText"/>
		<rdfs:seeAlso rdf:resource="#JavaLang"/>
		<rdfs:seeAlso rdf:resource="#JavaAwtFont"/>
		<rdfs:seeAlso rdf:resource="#JavaxAccessibility"/>
		<rdfs:comment xml:lang="en">Java API part implementing the java.awt package for J2SE 1.3</rdfs:comment>
	</owl:Class>
	<owl:Class rdf:about="#JavaAwtGeom">
		<rdfs:subClassOf rdf:resource="&j2se-1_2;JavaAwtGeom"/>
		<rdfs:seeAlso rdf:resource="#JavaAwt"/>
		<rdfs:seeAlso rdf:resource="#JavaLang"/>
		<rdfs:seeAlso rdf:resource="#JavaIo"/>
		<rdfs:comment xml:lang="en">Java API part implementing the java.awt.geom package for J2SE 1.3</rdfs:comment>
	</owl:Class>
	<owl:Class rdf:about="#JavaAwtEvent">
		<rdfs:subClassOf rdf:resource="&j2me-pp-1_0;JavaAwtEvent"/>
		<rdfs:subClassOf rdf:resource="&j2se-1_2;JavaAwtEvent"/>
		<rdfs:seeAlso rdf:resource="#JavaText"/>
		<rdfs:seeAlso rdf:resource="#JavaUtil"/>
		<rdfs:seeAlso rdf:resource="#JavaAwt"/>
		<rdfs:seeAlso rdf:resource="#JavaLang"/>
		<rdfs:seeAlso rdf:resource="#JavaAwtFont"/>
		<rdfs:comment xml:lang="en">Java API part implementing the java.awt.event package for J2SE 1.3</rdfs:comment>
	</owl:Class>
	<owl:Class rdf:about="#JavaAwtFont">
		<rdfs:subClassOf rdf:resource="&java;JavaAPIPart"/>
		<rdfs:seeAlso rdf:resource="#JavaAwtGeom"/>
		<rdfs:seeAlso rdf:resource="#JavaIo"/>
		<rdfs:seeAlso rdf:resource="#JavaText"/>
		<rdfs:seeAlso rdf:resource="#JavaUtil"/>
		<rdfs:seeAlso rdf:resource="#JavaAwt"/>
		<rdfs:seeAlso rdf:resource="#JavaLang"/>
		<rdfs:comment xml:lang="en">Java API part implementing the java.awt.font package for J2SE 1.3</rdfs:comment>
	</owl:Class>
	<owl:Class rdf:about="#JavaAwtImage">
		<rdfs:subClassOf rdf:resource="&j2me-pp-1_0;JavaAwtImage"/>
		<rdfs:subClassOf rdf:resource="&j2se-1_2;JavaAwtImage"/>
		<rdfs:seeAlso rdf:resource="#JavaAwtGeom"/>
		<rdfs:seeAlso rdf:resource="#JavaMath"/>
		<rdfs:seeAlso rdf:resource="#JavaUtil"/>
		<rdfs:seeAlso rdf:resource="#JavaAwt"/>
		<rdfs:seeAlso rdf:resource="#JavaAwtColor"/>
		<rdfs:seeAlso rdf:resource="#JavaLang"/>
		<rdfs:comment xml:lang="en">Java API part implementing the java.awt.image package for J2SE 1.3</rdfs:comment>
	</owl:Class>
	<owl:Class rdf:about="#JavaAwtImageRenderable">
		<rdfs:subClassOf rdf:resource="&j2se-1_2;JavaAwtImageRenderable"/>
		<rdfs:seeAlso rdf:resource="#JavaAwtGeom"/>
		<rdfs:seeAlso rdf:resource="#JavaIo"/>
		<rdfs:seeAlso rdf:resource="#JavaUtil"/>
		<rdfs:seeAlso rdf:resource="#JavaAwtImage"/>
		<rdfs:seeAlso rdf:resource="#JavaAwt"/>
		<rdfs:seeAlso rdf:resource="#JavaLang"/>
		<rdfs:comment xml:lang="en">Java API part implementing the java.awt.image.renderable package for J2SE 1.3</rdfs:comment>
	</owl:Class>
	<owl:Class rdf:about="#JavaAwtDnd">
		<owl:equivalentClass rdf:resource="&j2se-1_2;JavaAwtDnd"/>
		<rdfs:subClassOf rdf:resource="&java;JavaAPIPart"/>
		<rdfs:seeAlso rdf:resource="#JavaIo"/>
		<rdfs:seeAlso rdf:resource="#JavaAwtEvent"/>
		<rdfs:seeAlso rdf:resource="#JavaUtil"/>
		<rdfs:seeAlso rdf:resource="#JavaAwt"/>
		<rdfs:seeAlso rdf:resource="#JavaLang"/>
		<rdfs:seeAlso rdf:resource="#JavaAwtDatatransfer"/>
		<rdfs:comment xml:lang="en">Java API part implementing the java.awt.dnd package for J2SE 1.3</rdfs:comment>
	</owl:Class>
	<owl:Class rdf:about="#JavaAwtIm">
		<rdfs:subClassOf rdf:resource="&j2se-1_2;JavaAwtIm"/>
		<rdfs:seeAlso rdf:resource="#JavaText"/>
		<rdfs:seeAlso rdf:resource="#JavaUtil"/>
		<rdfs:seeAlso rdf:resource="#JavaAwt"/>
		<rdfs:seeAlso rdf:resource="#JavaLang"/>
		<rdfs:seeAlso rdf:resource="#JavaAwtFont"/>
		<rdfs:comment xml:lang="en">Java API part implementing the java.awt.im package for J2SE 1.3</rdfs:comment>
	</owl:Class>
	<owl:Class rdf:about="#JavaAwtImSpi">
		<rdfs:subClassOf rdf:resource="&java;JavaAPIPart"/>
		<rdfs:seeAlso rdf:resource="#JavaText"/>
		<rdfs:seeAlso rdf:resource="#JavaUtil"/>
		<rdfs:seeAlso rdf:resource="#JavaAwt"/>
		<rdfs:seeAlso rdf:resource="#JavaLang"/>
		<rdfs:seeAlso rdf:resource="#JavaAwtFont"/>
		<rdfs:seeAlso rdf:resource="#JavaAwtIm"/>
		<rdfs:comment xml:lang="en">Java API part implementing the java.awt.im.spi package for J2SE 1.3</rdfs:comment>
	</owl:Class>
	<owl:Class rdf:about="#JavaAwtColor">
		<rdfs:subClassOf rdf:resource="&j2me-pp-1_0;JavaAwtColor"/>
		<rdfs:subClassOf rdf:resource="&j2se-1_2;JavaAwtColor"/>
		<rdfs:seeAlso rdf:resource="#JavaLang"/>
		<rdfs:seeAlso rdf:resource="#JavaIo"/>
		<rdfs:comment xml:lang="en">Java API part implementing the java.awt.color package for J2SE 1.3</rdfs:comment>
	</owl:Class>
	<owl:Class rdf:about="#JavaAwtDatatransfer">
		<rdfs:subClassOf rdf:resource="&j2me-pp-1_0;JavaAwtDatatransfer"/>
		<rdfs:subClassOf rdf:resource="&j2se-1_2;JavaAwtDatatransfer"/>
		<rdfs:seeAlso rdf:resource="#JavaUtil"/>
		<rdfs:seeAlso rdf:resource="#JavaLang"/>
		<rdfs:seeAlso rdf:resource="#JavaIo"/>
		<rdfs:comment xml:lang="en">Java API part implementing the java.awt.datatransfer package for J2SE 1.3</rdfs:comment>
	</owl:Class>
	<owl:Class rdf:about="#JavaAwtPrint">
		<owl:equivalentClass rdf:resource="&j2se-1_2;JavaAwtPrint"/>
		<rdfs:subClassOf rdf:resource="&java;JavaAPIPart"/>
		<rdfs:seeAlso rdf:resource="#JavaAwt"/>
		<rdfs:seeAlso rdf:resource="#JavaLang"/>
		<rdfs:seeAlso rdf:resource="#JavaIo"/>
		<rdfs:comment xml:lang="en">Java API part implementing the java.awt.print package for J2SE 1.3</rdfs:comment>
	</owl:Class>
	<owl:Class rdf:about="#JavaBeans">
		<owl:equivalentClass rdf:resource="&j2se-1_2;JavaBeans"/>
		<rdfs:subClassOf rdf:resource="&j2me-pp-1_0;JavaBeans"/>
		<rdfs:seeAlso rdf:resource="#JavaLangReflect"/>
		<rdfs:seeAlso rdf:resource="#JavaBeansBeancontext"/>
		<rdfs:seeAlso rdf:resource="#JavaIo"/>
		<rdfs:seeAlso rdf:resource="#JavaUtil"/>
		<rdfs:seeAlso rdf:resource="#JavaAwt"/>
		<rdfs:seeAlso rdf:resource="#JavaApplet"/>
		<rdfs:seeAlso rdf:resource="#JavaLang"/>
		<rdfs:comment xml:lang="en">Java API part implementing the java.beans package for J2SE 1.3</rdfs:comment>
	</owl:Class>
	<owl:Class rdf:about="#JavaBeansBeancontext">
		<owl:equivalentClass rdf:resource="&j2se-1_2;JavaBeansBeancontext"/>
		<rdfs:subClassOf rdf:resource="&java;JavaAPIPart"/>
		<rdfs:seeAlso rdf:resource="#JavaBeans"/>
		<rdfs:seeAlso rdf:resource="#JavaIo"/>
		<rdfs:seeAlso rdf:resource="#JavaUtil"/>
		<rdfs:seeAlso rdf:resource="#JavaAwt"/>
		<rdfs:seeAlso rdf:resource="#JavaNet"/>
		<rdfs:seeAlso rdf:resource="#JavaLang"/>
		<rdfs:comment xml:lang="en">Java API part implementing the java.beans.beancontext package for J2SE 1.3</rdfs:comment>
	</owl:Class>
	<owl:Class rdf:about="#JavaApplet">
		<rdfs:subClassOf rdf:resource="&j2me-pp-1_0;JavaApplet"/>
		<rdfs:subClassOf rdf:resource="&j2se-1_2;JavaApplet"/>
		<rdfs:seeAlso rdf:resource="#JavaxAccessibility"/>
		<rdfs:seeAlso rdf:resource="#JavaUtil"/>
		<rdfs:seeAlso rdf:resource="#JavaAwt"/>
		<rdfs:seeAlso rdf:resource="#JavaNet"/>
		<rdfs:seeAlso rdf:resource="#JavaLang"/>
		<rdfs:comment xml:lang="en">Java API part implementing the java.applet package for J2SE 1.3</rdfs:comment>
	</owl:Class>
	<owl:Class rdf:about="#JavaRmi">
		<owl:equivalentClass rdf:resource="&j2se-1_2;JavaRmi"/>
		<rdfs:subClassOf rdf:resource="&j2me-pp-1_0;JavaRmi"/>
		<rdfs:seeAlso rdf:resource="#JavaLang"/>
		<rdfs:seeAlso rdf:resource="#JavaIo"/>
		<rdfs:comment xml:lang="en">Java API part implementing the java.rmi package for J2SE 1.3</rdfs:comment>
	</owl:Class>
	<owl:Class rdf:about="#JavaRmiServer">
		<rdfs:subClassOf rdf:resource="&j2se-1_2;JavaRmiServer"/>
		<rdfs:seeAlso rdf:resource="#JavaLangReflect"/>
		<rdfs:seeAlso rdf:resource="#JavaIo"/>
		<rdfs:seeAlso rdf:resource="#JavaRmi"/>
		<rdfs:seeAlso rdf:resource="#JavaNet"/>
		<rdfs:seeAlso rdf:resource="#JavaLang"/>
		<rdfs:comment xml:lang="en">Java API part implementing the java.rmi.server package for J2SE 1.3</rdfs:comment>
	</owl:Class>
	<owl:Class rdf:about="#JavaRmiDgc">
		<owl:equivalentClass rdf:resource="&j2se-1_2;JavaRmiDgc"/>
		<rdfs:subClassOf rdf:resource="&java;JavaAPIPart"/>
		<rdfs:seeAlso rdf:resource="#JavaRmi"/>
		<rdfs:seeAlso rdf:resource="#JavaLang"/>
		<rdfs:seeAlso rdf:resource="#JavaIo"/>
		<rdfs:comment xml:lang="en">Java API part implementing the java.rmi.dgc package for J2SE 1.3</rdfs:comment>
	</owl:Class>
	<owl:Class rdf:about="#JavaRmiRegistry">
		<owl:equivalentClass rdf:resource="&j2se-1_2;JavaRmiRegistry"/>
		<rdfs:subClassOf rdf:resource="&j2me-pp-1_0;JavaRmiRegistry"/>
		<rdfs:seeAlso rdf:resource="#JavaRmi"/>
		<rdfs:seeAlso rdf:resource="#JavaRmiServer"/>
		<rdfs:seeAlso rdf:resource="#JavaLang"/>
		<rdfs:comment xml:lang="en">Java API part implementing the java.rmi.registry package for J2SE 1.3</rdfs:comment>
	</owl:Class>
	<owl:Class rdf:about="#JavaRmiActivation">
		<owl:equivalentClass rdf:resource="&j2se-1_2;JavaRmiActivation"/>
		<rdfs:subClassOf rdf:resource="&java;JavaAPIPart"/>
		<rdfs:seeAlso rdf:resource="#JavaIo"/>
		<rdfs:seeAlso rdf:resource="#JavaRmi"/>
		<rdfs:seeAlso rdf:resource="#JavaRmiServer"/>
		<rdfs:seeAlso rdf:resource="#JavaUtil"/>
		<rdfs:seeAlso rdf:resource="#JavaLang"/>
		<rdfs:comment xml:lang="en">Java API part implementing the java.rmi.activation package for J2SE 1.3</rdfs:comment>
	</owl:Class>
	<owl:Class rdf:about="#JavaSql">
		<rdfs:subClassOf rdf:resource="&j2se-1_2;JavaSql"/>
		<rdfs:seeAlso rdf:resource="#JavaIo"/>
		<rdfs:seeAlso rdf:resource="#JavaSecurity"/>
		<rdfs:seeAlso rdf:resource="#JavaMath"/>
		<rdfs:seeAlso rdf:resource="#JavaUtil"/>
		<rdfs:seeAlso rdf:resource="#JavaLang"/>
		<rdfs:comment xml:lang="en">Java API part implementing the java.sql package for J2SE 1.3</rdfs:comment>
	</owl:Class>
	<owl:Class rdf:about="#JavaxAccessibility">
		<rdfs:subClassOf rdf:resource="&j2se-1_2;JavaxAccessibility"/>
		<rdfs:seeAlso rdf:resource="#JavaBeans"/>
		<rdfs:seeAlso rdf:resource="#JavaAwtEvent"/>
		<rdfs:seeAlso rdf:resource="#JavaxSwingText"/>
		<rdfs:seeAlso rdf:resource="#JavaUtil"/>
		<rdfs:seeAlso rdf:resource="#JavaAwt"/>
		<rdfs:seeAlso rdf:resource="#JavaLang"/>
		<rdfs:comment xml:lang="en">Java API part implementing the javax.accessibility package for J2SE 1.3</rdfs:comment>
	</owl:Class>
	<owl:Class rdf:about="#JavaxSwing">
		<rdfs:subClassOf rdf:resource="&java;JavaAPIPart"/>
		<rdfs:seeAlso rdf:resource="#JavaBeans"/>
		<rdfs:seeAlso rdf:resource="#JavaIo"/>
		<rdfs:seeAlso rdf:resource="#JavaAwtEvent"/>
		<rdfs:seeAlso rdf:resource="#JavaApplet"/>
		<rdfs:seeAlso rdf:resource="#JavaxSwingTable"/>
		<rdfs:seeAlso rdf:resource="#JavaText"/>
		<rdfs:seeAlso rdf:resource="#JavaAwt"/>
		<rdfs:seeAlso rdf:resource="#JavaxSwingColorchooser"/>
		<rdfs:seeAlso rdf:resource="#JavaxAccessibility"/>
		<rdfs:seeAlso rdf:resource="#JavaxSwingPlaf"/>
		<rdfs:seeAlso rdf:resource="#JavaxSwingText"/>
		<rdfs:seeAlso rdf:resource="#JavaUtil"/>
		<rdfs:seeAlso rdf:resource="#JavaxSwingTree"/>
		<rdfs:seeAlso rdf:resource="#JavaNet"/>
		<rdfs:seeAlso rdf:resource="#JavaxSwingBorder"/>
		<rdfs:seeAlso rdf:resource="#JavaxSwingEvent"/>
		<rdfs:seeAlso rdf:resource="#JavaAwtImage"/>
		<rdfs:seeAlso rdf:resource="#JavaLang"/>
		<rdfs:seeAlso rdf:resource="#JavaxSwingFilechooser"/>
		<rdfs:comment xml:lang="en">Java API part implementing the javax.swing package for J2SE 1.3</rdfs:comment>
	</owl:Class>
	<owl:Class rdf:about="#JavaxSwingText">
		<rdfs:subClassOf rdf:resource="&j2se-1_2;JavaxSwingText"/>
		<rdfs:seeAlso rdf:resource="#JavaIo"/>
		<rdfs:seeAlso rdf:resource="#JavaAwtEvent"/>
		<rdfs:seeAlso rdf:resource="#JavaxSwingPlaf"/>
		<rdfs:seeAlso rdf:resource="#JavaUtil"/>
		<rdfs:seeAlso rdf:resource="#JavaxSwingTree"/>
		<rdfs:seeAlso rdf:resource="#JavaAwtIm"/>
		<rdfs:seeAlso rdf:resource="#JavaxSwingEvent"/>
		<rdfs:seeAlso rdf:resource="#JavaxSwingPlafBasic"/>
		<rdfs:seeAlso rdf:resource="#JavaText"/>
		<rdfs:seeAlso rdf:resource="#JavaAwt"/>
		<rdfs:seeAlso rdf:resource="#JavaLang"/>
		<rdfs:seeAlso rdf:resource="#JavaxSwing"/>
		<rdfs:seeAlso rdf:resource="#JavaxSwingUndo"/>
		<rdfs:seeAlso rdf:resource="#JavaxAccessibility"/>
		<rdfs:comment xml:lang="en">Java API part implementing the javax.swing.text package for J2SE 1.3</rdfs:comment>
	</owl:Class>
	<owl:Class rdf:about="#JavaxSwingTextHtml">
		<rdfs:subClassOf rdf:resource="&j2se-1_2;JavaxSwingTextHtml"/>
		<rdfs:seeAlso rdf:resource="#JavaIo"/>
		<rdfs:seeAlso rdf:resource="#JavaAwtEvent"/>
		<rdfs:seeAlso rdf:resource="#JavaxSwingText"/>
		<rdfs:seeAlso rdf:resource="#JavaUtil"/>
		<rdfs:seeAlso rdf:resource="#JavaNet"/>
		<rdfs:seeAlso rdf:resource="#JavaxSwingEvent"/>
		<rdfs:seeAlso rdf:resource="#JavaAwt"/>
		<rdfs:seeAlso rdf:resource="#JavaLang"/>
		<rdfs:seeAlso rdf:resource="#JavaxSwing"/>
		<rdfs:comment xml:lang="en">Java API part implementing the javax.swing.text.html package for J2SE 1.3</rdfs:comment>
	</owl:Class>
	<owl:Class rdf:about="#JavaxSwingTextHtmlParser">
		<rdfs:subClassOf rdf:resource="&j2se-1_2;JavaxSwingTextHtmlParser"/>
		<rdfs:seeAlso rdf:resource="#JavaIo"/>
		<rdfs:seeAlso rdf:resource="#JavaxSwingTextHtml"/>
		<rdfs:seeAlso rdf:resource="#JavaxSwingText"/>
		<rdfs:seeAlso rdf:resource="#JavaUtil"/>
		<rdfs:seeAlso rdf:resource="#JavaLang"/>
		<rdfs:comment xml:lang="en">Java API part implementing the javax.swing.text.html.parser package for J2SE 1.3</rdfs:comment>
	</owl:Class>
	<owl:Class rdf:about="#JavaxSwingTextRtf">
		<owl:equivalentClass rdf:resource="&j2se-1_2;JavaxSwingTextRtf"/>
		<rdfs:subClassOf rdf:resource="&java;JavaAPIPart"/>
		<rdfs:seeAlso rdf:resource="#JavaxSwingText"/>
		<rdfs:seeAlso rdf:resource="#JavaLang"/>
		<rdfs:seeAlso rdf:resource="#JavaIo"/>
		<rdfs:comment xml:lang="en">Java API part implementing the javax.swing.text.rtf package for J2SE 1.3</rdfs:comment>
	</owl:Class>
	<owl:Class rdf:about="#JavaxSwingEvent">
		<rdfs:subClassOf rdf:resource="&j2se-1_2;JavaxSwingEvent"/>
		<rdfs:seeAlso rdf:resource="#JavaxSwingTable"/>
		<rdfs:seeAlso rdf:resource="#JavaBeans"/>
		<rdfs:seeAlso rdf:resource="#JavaIo"/>
		<rdfs:seeAlso rdf:resource="#JavaAwtEvent"/>
		<rdfs:seeAlso rdf:resource="#JavaxSwingText"/>
		<rdfs:seeAlso rdf:resource="#JavaUtil"/>
		<rdfs:seeAlso rdf:resource="#JavaAwt"/>
		<rdfs:seeAlso rdf:resource="#JavaxSwingTree"/>
		<rdfs:seeAlso rdf:resource="#JavaNet"/>
		<rdfs:seeAlso rdf:resource="#JavaLang"/>
		<rdfs:seeAlso rdf:resource="#JavaxSwing"/>
		<rdfs:seeAlso rdf:resource="#JavaxSwingUndo"/>
		<rdfs:comment xml:lang="en">Java API part implementing the javax.swing.event package for J2SE 1.3</rdfs:comment>
	</owl:Class>
	<owl:Class rdf:about="#JavaxSwingPlaf">
		<rdfs:subClassOf rdf:resource="&j2se-1_2;JavaxSwingPlaf"/>
		<rdfs:seeAlso rdf:resource="#JavaIo"/>
		<rdfs:seeAlso rdf:resource="#JavaAwtEvent"/>
		<rdfs:seeAlso rdf:resource="#JavaxSwingText"/>
		<rdfs:seeAlso rdf:resource="#JavaAwt"/>
		<rdfs:seeAlso rdf:resource="#JavaxSwingTree"/>
		<rdfs:seeAlso rdf:resource="#JavaLang"/>
		<rdfs:seeAlso rdf:resource="#JavaxSwingBorder"/>
		<rdfs:seeAlso rdf:resource="#JavaxSwingFilechooser"/>
		<rdfs:seeAlso rdf:resource="#JavaxSwing"/>
		<rdfs:seeAlso rdf:resource="#JavaxAccessibility"/>
		<rdfs:comment xml:lang="en">Java API part implementing the javax.swing.plaf package for J2SE 1.3</rdfs:comment>
	</owl:Class>
	<owl:Class rdf:about="#JavaxSwingPlafBasic">
		<rdfs:subClassOf rdf:resource="&j2se-1_2;JavaxSwingPlafBasic"/>
		<rdfs:seeAlso rdf:resource="#JavaBeans"/>
		<rdfs:seeAlso rdf:resource="#JavaIo"/>
		<rdfs:seeAlso rdf:resource="#JavaAwtEvent"/>
		<rdfs:seeAlso rdf:resource="#JavaxSwingTable"/>
		<rdfs:seeAlso rdf:resource="#JavaAwt"/>
		<rdfs:seeAlso rdf:resource="#JavaxAccessibility"/>
		<rdfs:seeAlso rdf:resource="#JavaxSwingPlaf"/>
		<rdfs:seeAlso rdf:resource="#JavaxSwingText"/>
		<rdfs:seeAlso rdf:resource="#JavaUtil"/>
		<rdfs:seeAlso rdf:resource="#JavaxSwingTree"/>
		<rdfs:seeAlso rdf:resource="#JavaxSwingBorder"/>
		<rdfs:seeAlso rdf:resource="#JavaxSwingEvent"/>
		<rdfs:seeAlso rdf:resource="#JavaLang"/>
		<rdfs:seeAlso rdf:resource="#JavaxSwingFilechooser"/>
		<rdfs:seeAlso rdf:resource="#JavaxSwing"/>
		<rdfs:comment xml:lang="en">Java API part implementing the javax.swing.plaf.basic package for J2SE 1.3</rdfs:comment>
	</owl:Class>
	<owl:Class rdf:about="#JavaxSwingPlafMetal">
		<rdfs:subClassOf rdf:resource="&j2se-1_2;JavaxSwingPlafMetal"/>
		<rdfs:seeAlso rdf:resource="#JavaBeans"/>
		<rdfs:seeAlso rdf:resource="#JavaIo"/>
		<rdfs:seeAlso rdf:resource="#JavaAwtEvent"/>
		<rdfs:seeAlso rdf:resource="#JavaxSwingPlaf"/>
		<rdfs:seeAlso rdf:resource="#JavaxSwingTree"/>
		<rdfs:seeAlso rdf:resource="#JavaxSwingBorder"/>
		<rdfs:seeAlso rdf:resource="#JavaxSwingEvent"/>
		<rdfs:seeAlso rdf:resource="#JavaxSwingPlafBasic"/>
		<rdfs:seeAlso rdf:resource="#JavaAwt"/>
		<rdfs:seeAlso rdf:resource="#JavaLang"/>
		<rdfs:seeAlso rdf:resource="#JavaxSwing"/>
		<rdfs:comment xml:lang="en">Java API part implementing the javax.swing.plaf.metal package for J2SE 1.3</rdfs:comment>
	</owl:Class>
	<owl:Class rdf:about="#JavaxSwingPlafMulti">
		<rdfs:subClassOf rdf:resource="&j2se-1_2;JavaxSwingPlafMulti"/>
		<rdfs:seeAlso rdf:resource="#JavaIo"/>
		<rdfs:seeAlso rdf:resource="#JavaxSwingPlaf"/>
		<rdfs:seeAlso rdf:resource="#JavaxSwingText"/>
		<rdfs:seeAlso rdf:resource="#JavaUtil"/>
		<rdfs:seeAlso rdf:resource="#JavaxSwingTree"/>
		<rdfs:seeAlso rdf:resource="#JavaAwt"/>
		<rdfs:seeAlso rdf:resource="#JavaLang"/>
		<rdfs:seeAlso rdf:resource="#JavaxSwingFilechooser"/>
		<rdfs:seeAlso rdf:resource="#JavaxSwing"/>
		<rdfs:seeAlso rdf:resource="#JavaxAccessibility"/>
		<rdfs:comment xml:lang="en">Java API part implementing the javax.swing.plaf.multi package for J2SE 1.3</rdfs:comment>
	</owl:Class>
	<owl:Class rdf:about="#JavaxSwingUndo">
		<owl:equivalentClass rdf:resource="&j2se-1_2;JavaxSwingUndo"/>
		<rdfs:subClassOf rdf:resource="&java;JavaAPIPart"/>
		<rdfs:seeAlso rdf:resource="#JavaxSwingEvent"/>
		<rdfs:seeAlso rdf:resource="#JavaUtil"/>
		<rdfs:seeAlso rdf:resource="#JavaLang"/>
		<rdfs:seeAlso rdf:resource="#JavaIo"/>
		<rdfs:comment xml:lang="en">Java API part implementing the javax.swing.undo package for J2SE 1.3</rdfs:comment>
	</owl:Class>
	<owl:Class rdf:about="#JavaxSwingTree">
		<rdfs:subClassOf rdf:resource="&j2se-1_2;JavaxSwingTree"/>
		<rdfs:seeAlso rdf:resource="#JavaBeans"/>
		<rdfs:seeAlso rdf:resource="#JavaIo"/>
		<rdfs:seeAlso rdf:resource="#JavaAwtEvent"/>
		<rdfs:seeAlso rdf:resource="#JavaUtil"/>
		<rdfs:seeAlso rdf:resource="#JavaAwt"/>
		<rdfs:seeAlso rdf:resource="#JavaLang"/>
		<rdfs:seeAlso rdf:resource="#JavaxSwingBorder"/>
		<rdfs:seeAlso rdf:resource="#JavaxSwingEvent"/>
		<rdfs:seeAlso rdf:resource="#JavaxSwing"/>
		<rdfs:comment xml:lang="en">Java API part implementing the javax.swing.tree package for J2SE 1.3</rdfs:comment>
	</owl:Class>
	<owl:Class rdf:about="#JavaxSwingTable">
		<rdfs:subClassOf rdf:resource="&j2se-1_2;JavaxSwingTable"/>
		<rdfs:seeAlso rdf:resource="#JavaBeans"/>
		<rdfs:seeAlso rdf:resource="#JavaIo"/>
		<rdfs:seeAlso rdf:resource="#JavaAwtEvent"/>
		<rdfs:seeAlso rdf:resource="#JavaxSwingPlaf"/>
		<rdfs:seeAlso rdf:resource="#JavaUtil"/>
		<rdfs:seeAlso rdf:resource="#JavaAwt"/>
		<rdfs:seeAlso rdf:resource="#JavaLang"/>
		<rdfs:seeAlso rdf:resource="#JavaxSwingBorder"/>
		<rdfs:seeAlso rdf:resource="#JavaxSwingEvent"/>
		<rdfs:seeAlso rdf:resource="#JavaxSwing"/>
		<rdfs:seeAlso rdf:resource="#JavaxAccessibility"/>
		<rdfs:comment xml:lang="en">Java API part implementing the javax.swing.table package for J2SE 1.3</rdfs:comment>
	</owl:Class>
	<owl:Class rdf:about="#JavaxSwingBorder">
		<rdfs:subClassOf rdf:resource="&j2se-1_2;JavaxSwingBorder"/>
		<rdfs:seeAlso rdf:resource="#JavaAwt"/>
		<rdfs:seeAlso rdf:resource="#JavaLang"/>
		<rdfs:seeAlso rdf:resource="#JavaxSwing"/>
		<rdfs:seeAlso rdf:resource="#JavaIo"/>
		<rdfs:comment xml:lang="en">Java API part implementing the javax.swing.border package for J2SE 1.3</rdfs:comment>
	</owl:Class>
	<owl:Class rdf:about="#JavaxSwingColorchooser">
		<rdfs:subClassOf rdf:resource="&j2se-1_2;JavaxSwingColorchooser"/>
		<rdfs:seeAlso rdf:resource="#JavaxSwingEvent"/>
		<rdfs:seeAlso rdf:resource="#JavaxSwing"/>
		<rdfs:seeAlso rdf:resource="#JavaIo"/>
		<rdfs:seeAlso rdf:resource="#JavaAwt"/>
		<rdfs:seeAlso rdf:resource="#JavaLang"/>
		<rdfs:comment xml:lang="en">Java API part implementing the javax.swing.colorchooser package for J2SE 1.3</rdfs:comment>
	</owl:Class>
	<owl:Class rdf:about="#JavaxSwingFilechooser">
		<rdfs:subClassOf rdf:resource="&j2se-1_2;JavaxSwingFilechooser"/>
		<rdfs:seeAlso rdf:resource="#JavaxSwing"/>
		<rdfs:seeAlso rdf:resource="#JavaLang"/>
		<rdfs:seeAlso rdf:resource="#JavaIo"/>
		<rdfs:comment xml:lang="en">Java API part implementing the javax.swing.filechooser package for J2SE 1.3</rdfs:comment>
	</owl:Class>
	<owl:Class rdf:about="#JavaxNaming">
		<rdfs:subClassOf rdf:resource="&java;JavaAPIPart"/>
		<rdfs:seeAlso rdf:resource="#JavaIo"/>
		<rdfs:seeAlso rdf:resource="#JavaUtil"/>
		<rdfs:seeAlso rdf:resource="#JavaLang"/>
		<rdfs:comment xml:lang="en">Java API part implementing the javax.naming package for J2SE 1.3</rdfs:comment>
	</owl:Class>
	<owl:Class rdf:about="#JavaxNamingDirectory">
		<rdfs:subClassOf rdf:resource="&java;JavaAPIPart"/>
		<rdfs:seeAlso rdf:resource="#JavaxNaming"/>
		<rdfs:seeAlso rdf:resource="#JavaIo"/>
		<rdfs:seeAlso rdf:resource="#JavaUtil"/>
		<rdfs:seeAlso rdf:resource="#JavaLang"/>
		<rdfs:comment xml:lang="en">Java API part implementing the javax.naming.directory package for J2SE 1.3</rdfs:comment>
	</owl:Class>
	<owl:Class rdf:about="#JavaxNamingEvent">
		<rdfs:subClassOf rdf:resource="&java;JavaAPIPart"/>
		<rdfs:seeAlso rdf:resource="#JavaxNamingDirectory"/>
		<rdfs:seeAlso rdf:resource="#JavaUtil"/>
		<rdfs:seeAlso rdf:resource="#JavaxNaming"/>
		<rdfs:seeAlso rdf:resource="#JavaLang"/>
		<rdfs:comment xml:lang="en">Java API part implementing the javax.naming.event package for J2SE 1.3</rdfs:comment>
	</owl:Class>
	<owl:Class rdf:about="#JavaxNamingLdap">
		<rdfs:subClassOf rdf:resource="&java;JavaAPIPart"/>
		<rdfs:seeAlso rdf:resource="#JavaxNamingDirectory"/>
		<rdfs:seeAlso rdf:resource="#JavaxNamingEvent"/>
		<rdfs:seeAlso rdf:resource="#JavaUtil"/>
		<rdfs:seeAlso rdf:resource="#JavaxNaming"/>
		<rdfs:seeAlso rdf:resource="#JavaLang"/>
		<rdfs:seeAlso rdf:resource="#JavaIo"/>
		<rdfs:comment xml:lang="en">Java API part implementing the javax.naming.ldap package for J2SE 1.3</rdfs:comment>
	</owl:Class>
	<owl:Class rdf:about="#JavaxNamingSpi">
		<rdfs:subClassOf rdf:resource="&java;JavaAPIPart"/>
		<rdfs:seeAlso rdf:resource="#JavaxNamingDirectory"/>
		<rdfs:seeAlso rdf:resource="#JavaUtil"/>
		<rdfs:seeAlso rdf:resource="#JavaxNaming"/>
		<rdfs:seeAlso rdf:resource="#JavaLang"/>
		<rdfs:seeAlso rdf:resource="#JavaIo"/>
		<rdfs:comment xml:lang="en">Java API part implementing the javax.naming.spi package for J2SE 1.3</rdfs:comment>
	</owl:Class>
	<owl:Class rdf:about="#JavaxSoundMidi">
		<rdfs:subClassOf rdf:resource="&java;JavaAPIPart"/>
		<rdfs:seeAlso rdf:resource="#JavaUtil"/>
		<rdfs:seeAlso rdf:resource="#JavaNet"/>
		<rdfs:seeAlso rdf:resource="#JavaLang"/>
		<rdfs:seeAlso rdf:resource="#JavaIo"/>
		<rdfs:comment xml:lang="en">Java API part implementing the javax.sound.midi package for J2SE 1.3</rdfs:comment>
	</owl:Class>
	<owl:Class rdf:about="#JavaxSoundMidiSpi">
		<rdfs:subClassOf rdf:resource="&java;JavaAPIPart"/>
		<rdfs:seeAlso rdf:resource="#JavaNet"/>
		<rdfs:seeAlso rdf:resource="#JavaLang"/>
		<rdfs:seeAlso rdf:resource="#JavaxSoundMidi"/>
		<rdfs:seeAlso rdf:resource="#JavaIo"/>
		<rdfs:comment xml:lang="en">Java API part implementing the javax.sound.midi.spi package for J2SE 1.3</rdfs:comment>
	</owl:Class>
	<owl:Class rdf:about="#JavaxSoundSampled">
		<rdfs:subClassOf rdf:resource="&java;JavaAPIPart"/>
		<rdfs:seeAlso rdf:resource="#JavaUtil"/>
		<rdfs:seeAlso rdf:resource="#JavaNet"/>
		<rdfs:seeAlso rdf:resource="#JavaLang"/>
		<rdfs:seeAlso rdf:resource="#JavaIo"/>
		<rdfs:seeAlso rdf:resource="#JavaSecurity"/>
		<rdfs:comment xml:lang="en">Java API part implementing the javax.sound.sampled package for J2SE 1.3</rdfs:comment>
	</owl:Class>
	<owl:Class rdf:about="#JavaxSoundSampledSpi">
		<rdfs:subClassOf rdf:resource="&java;JavaAPIPart"/>
		<rdfs:seeAlso rdf:resource="#JavaIo"/>
		<rdfs:seeAlso rdf:resource="#JavaNet"/>
		<rdfs:seeAlso rdf:resource="#JavaLang"/>
		<rdfs:seeAlso rdf:resource="#JavaxSoundSampled"/>
		<rdfs:comment xml:lang="en">Java API part implementing the javax.sound.sampled.spi package for J2SE 1.3</rdfs:comment>
	</owl:Class>
	<owl:Class rdf:about="#JavaxRmi">
		<rdfs:subClassOf rdf:resource="&java;JavaAPIPart"/>
		<rdfs:seeAlso rdf:resource="#JavaRmi"/>
		<rdfs:seeAlso rdf:resource="#JavaLang"/>
		<rdfs:comment xml:lang="en">Java API part implementing the javax.rmi package for J2SE 1.3</rdfs:comment>
	</owl:Class>
	<owl:Class rdf:about="#JavaxRmiCORBA">
		<rdfs:subClassOf rdf:resource="&java;JavaAPIPart"/>
		<rdfs:seeAlso rdf:resource="#OrgOmgCORBAPortable"/>
		<rdfs:seeAlso rdf:resource="#OrgOmgCORBA_2_3Portable"/>
		<rdfs:seeAlso rdf:resource="#JavaIo"/>
		<rdfs:seeAlso rdf:resource="#OrgOmgSendingContext"/>
		<rdfs:seeAlso rdf:resource="#OrgOmgCORBA"/>
		<rdfs:seeAlso rdf:resource="#JavaRmi"/>
		<rdfs:seeAlso rdf:resource="#JavaLang"/>
		<rdfs:comment xml:lang="en">Java API part implementing the javax.rmi.CORBA package for J2SE 1.3</rdfs:comment>
	</owl:Class>
	<owl:Class rdf:about="#JavaxTransaction">
		<rdfs:subClassOf rdf:resource="&java;JavaAPIPart"/>
		<rdfs:seeAlso rdf:resource="#JavaRmi"/>
		<rdfs:seeAlso rdf:resource="#JavaLang"/>
		<rdfs:comment xml:lang="en">Java API part implementing the javax.transaction package for J2SE 1.3</rdfs:comment>
	</owl:Class>
	<owl:Class rdf:about="#OrgOmgCORBA_2_3">
		<rdfs:subClassOf rdf:resource="&java;JavaAPIPart"/>
		<rdfs:seeAlso rdf:resource="#OrgOmgCORBAPortable"/>
		<rdfs:seeAlso rdf:resource="#JavaLang"/>
		<rdfs:seeAlso rdf:resource="#OrgOmgCORBA"/>
		<rdfs:comment xml:lang="en">Java API part implementing the org.omg.CORBA_2_3 package for J2SE 1.3</rdfs:comment>
	</owl:Class>
	<owl:Class rdf:about="#OrgOmgCORBA_2_3Portable">
		<rdfs:subClassOf rdf:resource="&java;JavaAPIPart"/>
		<rdfs:seeAlso rdf:resource="#OrgOmgCORBAPortable"/>
		<rdfs:seeAlso rdf:resource="#JavaLang"/>
		<rdfs:seeAlso rdf:resource="#JavaIo"/>
		<rdfs:seeAlso rdf:resource="#OrgOmgCORBA"/>
		<rdfs:comment xml:lang="en">Java API part implementing the org.omg.CORBA_2_3.portable package for J2SE 1.3</rdfs:comment>
	</owl:Class>
	<owl:Class rdf:about="#OrgOmgCORBA">
		<rdfs:subClassOf rdf:resource="&j2se-1_2;OrgOmgCORBA"/>
		<rdfs:seeAlso rdf:resource="#OrgOmgCORBAPortable"/>
		<rdfs:seeAlso rdf:resource="#JavaIo"/>
		<rdfs:seeAlso rdf:resource="#JavaMath"/>
		<rdfs:seeAlso rdf:resource="#JavaUtil"/>
		<rdfs:seeAlso rdf:resource="#JavaApplet"/>
		<rdfs:seeAlso rdf:resource="#JavaLang"/>
		<rdfs:comment xml:lang="en">Java API part implementing the org.omg.CORBA package for J2SE 1.3</rdfs:comment>
	</owl:Class>
	<owl:Class rdf:about="#OrgOmgCORBAPortable">
		<rdfs:subClassOf rdf:resource="&j2se-1_2;OrgOmgCORBAPortable"/>
		<rdfs:seeAlso rdf:resource="#JavaIo"/>
		<rdfs:seeAlso rdf:resource="#JavaLang"/>
		<rdfs:seeAlso rdf:resource="#OrgOmgCORBA_2_3Portable"/>
		<rdfs:seeAlso rdf:resource="#OrgOmgCORBA"/>
		<rdfs:seeAlso rdf:resource="#JavaMath"/>
		<rdfs:comment xml:lang="en">Java API part implementing the org.omg.CORBA.portable package for J2SE 1.3</rdfs:comment>
	</owl:Class>
	<owl:Class rdf:about="#OrgOmgCORBATypeCodePackage">
		<owl:equivalentClass rdf:resource="&j2se-1_2;OrgOmgCORBATypeCodePackage"/>
		<rdfs:subClassOf rdf:resource="&java;JavaAPIPart"/>
		<rdfs:seeAlso rdf:resource="#JavaLang"/>
		<rdfs:seeAlso rdf:resource="#OrgOmgCORBA"/>
		<rdfs:comment xml:lang="en">Java API part implementing the org.omg.CORBA.TypeCodePackage package for J2SE 1.3</rdfs:comment>
	</owl:Class>
	<owl:Class rdf:about="#OrgOmgCORBAORBPackage">
		<owl:equivalentClass rdf:resource="&j2se-1_2;OrgOmgCORBAORBPackage"/>
		<rdfs:subClassOf rdf:resource="&java;JavaAPIPart"/>
		<rdfs:seeAlso rdf:resource="#JavaLang"/>
		<rdfs:seeAlso rdf:resource="#OrgOmgCORBA"/>
		<rdfs:comment xml:lang="en">Java API part implementing the org.omg.CORBA.ORBPackage package for J2SE 1.3</rdfs:comment>
	</owl:Class>
	<owl:Class rdf:about="#OrgOmgCORBADynAnyPackage">
		<owl:equivalentClass rdf:resource="&j2se-1_2;OrgOmgCORBADynAnyPackage"/>
		<rdfs:subClassOf rdf:resource="&java;JavaAPIPart"/>
		<rdfs:seeAlso rdf:resource="#JavaLang"/>
		<rdfs:seeAlso rdf:resource="#OrgOmgCORBA"/>
		<rdfs:comment xml:lang="en">Java API part implementing the org.omg.CORBA.DynAnyPackage package for J2SE 1.3</rdfs:comment>
	</owl:Class>
	<owl:Class rdf:about="#OrgOmgSendingContext">
		<rdfs:subClassOf rdf:resource="&java;JavaAPIPart"/>
		<rdfs:seeAlso rdf:resource="#OrgOmgCORBAPortable"/>
		<rdfs:seeAlso rdf:resource="#OrgOmgCORBA"/>
		<rdfs:comment xml:lang="en">Java API part implementing the org.omg.SendingContext package for J2SE 1.3</rdfs:comment>
	</owl:Class>
	<owl:Class rdf:about="#OrgOmgCosNaming">
		<rdfs:subClassOf rdf:resource="&j2se-1_2;OrgOmgCosNaming"/>
		<rdfs:seeAlso rdf:resource="#OrgOmgCORBAPortable"/>
		<rdfs:seeAlso rdf:resource="#OrgOmgCORBA"/>
		<rdfs:seeAlso rdf:resource="#JavaLang"/>
		<rdfs:comment xml:lang="en">Java API part implementing the org.omg.CosNaming package for J2SE 1.3</rdfs:comment>
	</owl:Class>
	<owl:Class rdf:about="#OrgOmgCosNamingNamingContextPackage">
		<owl:equivalentClass rdf:resource="&j2se-1_2;OrgOmgCosNamingNamingContextPackage"/>
		<rdfs:subClassOf rdf:resource="&java;JavaAPIPart"/>
		<rdfs:seeAlso rdf:resource="#OrgOmgCORBAPortable"/>
		<rdfs:seeAlso rdf:resource="#OrgOmgCosNaming"/>
		<rdfs:seeAlso rdf:resource="#JavaLang"/>
		<rdfs:seeAlso rdf:resource="#OrgOmgCORBA"/>
		<rdfs:comment xml:lang="en">Java API part implementing the org.omg.CosNaming.NamingContextPackage package for J2SE 1.3</rdfs:comment>
	</owl:Class>
	<owl:Class rdf:about="#OrgOmgStubJavaRmi">
		<rdfs:subClassOf rdf:resource="&java;JavaAPIPart"/>
		<rdfs:seeAlso rdf:resource="#JavaRmi"/>
		<rdfs:seeAlso rdf:resource="#JavaxRmiCORBA"/>
		<rdfs:comment xml:lang="en">Java API part implementing the org.omg.stub.java.rmi package for J2SE 1.3</rdfs:comment>
	</owl:Class>
	<owl:Class rdf:about="#JavaIoAPI">
		<rdfs:subClassOf rdf:resource="&j2me-pp-1_0;JavaIoAPI"/>
		<rdfs:subClassOf rdf:resource="&j2se-1_2;JavaIoAPI"/>
		<rdfs:comment xml:lang="en">JavaLibrary implementing the java.io package for J2SE 1.3</rdfs:comment>
		<rdfs:comment xml:lang="OWLManchester">platform:comprisesInterfacePart some JavaIo</rdfs:comment>
	</owl:Class>
	<owl:Class rdf:about="#JavaLangAPI">
		<rdfs:subClassOf rdf:resource="&j2me-pp-1_0;JavaLangAPI"/>
		<rdfs:subClassOf rdf:resource="&j2se-1_2;JavaLangAPI"/>
		<rdfs:comment xml:lang="en">JavaLibrary implementing the java.lang package for J2SE 1.3</rdfs:comment>
		<rdfs:comment xml:lang="OWLManchester">platform:comprisesInterfacePart some JavaLang</rdfs:comment>
	</owl:Class>
	<owl:Class rdf:about="#JavaLangReflectAPI">
		<owl:equivalentClass rdf:resource="&j2me-pp-1_0;JavaLangReflectAPI"/>
		<rdfs:subClassOf rdf:resource="&j2se-1_2;JavaLangReflectAPI"/>
		<rdfs:comment xml:lang="en">JavaLibrary implementing the java.lang.reflect package for J2SE 1.3</rdfs:comment>
		<rdfs:comment xml:lang="OWLManchester">platform:comprisesInterfacePart some JavaLangReflect</rdfs:comment>
	</owl:Class>
	<owl:Class rdf:about="#JavaLangRefAPI">
		<owl:equivalentClass rdf:resource="&j2me-pp-1_0;JavaLangRefAPI"/>
		<owl:equivalentClass rdf:resource="&j2se-1_2;JavaLangRefAPI"/>
		<rdfs:subClassOf rdf:resource="&java;JavaAPI"/>
		<rdfs:comment xml:lang="en">JavaLibrary implementing the java.lang.ref package for J2SE 1.3</rdfs:comment>
		<rdfs:comment xml:lang="OWLManchester">platform:comprisesInterfacePart some JavaLangRef</rdfs:comment>
	</owl:Class>
	<owl:Class rdf:about="#JavaNetAPI">
		<rdfs:subClassOf rdf:resource="&j2me-pp-1_0;JavaNetAPI"/>
		<rdfs:subClassOf rdf:resource="&j2se-1_2;JavaNetAPI"/>
		<rdfs:comment xml:lang="en">JavaLibrary implementing the java.net package for J2SE 1.3</rdfs:comment>
		<rdfs:comment xml:lang="OWLManchester">platform:comprisesInterfacePart some JavaNet</rdfs:comment>
	</owl:Class>
	<owl:Class rdf:about="#JavaSecurityAPI">
		<rdfs:subClassOf rdf:resource="&j2me-pp-1_0;JavaSecurityAPI"/>
		<rdfs:subClassOf rdf:resource="&j2se-1_2;JavaSecurityAPI"/>
		<rdfs:comment xml:lang="en">JavaLibrary implementing the java.security package for J2SE 1.3</rdfs:comment>
		<rdfs:comment xml:lang="OWLManchester">platform:comprisesInterfacePart some JavaSecurity</rdfs:comment>
	</owl:Class>
	<owl:Class rdf:about="#JavaSecurityCertAPI">
		<owl:equivalentClass rdf:resource="&j2me-pp-1_0;JavaSecurityCertAPI"/>
		<rdfs:subClassOf rdf:resource="&j2se-1_2;JavaSecurityCertAPI"/>
		<rdfs:comment xml:lang="en">JavaLibrary implementing the java.security.cert package for J2SE 1.3</rdfs:comment>
		<rdfs:comment xml:lang="OWLManchester">platform:comprisesInterfacePart some JavaSecurityCert</rdfs:comment>
	</owl:Class>
	<owl:Class rdf:about="#JavaSecuritySpecAPI">
		<owl:equivalentClass rdf:resource="&j2me-pp-1_0;JavaSecuritySpecAPI"/>
		<rdfs:subClassOf rdf:resource="&j2se-1_2;JavaSecuritySpecAPI"/>
		<rdfs:comment xml:lang="en">JavaLibrary implementing the java.security.spec package for J2SE 1.3</rdfs:comment>
		<rdfs:comment xml:lang="OWLManchester">platform:comprisesInterfacePart some JavaSecuritySpec</rdfs:comment>
	</owl:Class>
	<owl:Class rdf:about="#JavaSecurityInterfacesAPI">
		<owl:equivalentClass rdf:resource="&j2me-pp-1_0;JavaSecurityInterfacesAPI"/>
		<rdfs:subClassOf rdf:resource="&j2se-1_2;JavaSecurityInterfacesAPI"/>
		<rdfs:comment xml:lang="en">JavaLibrary implementing the java.security.interfaces package for J2SE 1.3</rdfs:comment>
		<rdfs:comment xml:lang="OWLManchester">platform:comprisesInterfacePart some JavaSecurityInterfaces</rdfs:comment>
	</owl:Class>
	<owl:Class rdf:about="#JavaSecurityAclAPI">
		<owl:equivalentClass rdf:resource="&j2me-pp-1_0;JavaSecurityAclAPI"/>
		<owl:equivalentClass rdf:resource="&j2se-1_2;JavaSecurityAclAPI"/>
		<rdfs:subClassOf rdf:resource="&java;JavaAPI"/>
		<rdfs:comment xml:lang="en">JavaLibrary implementing the java.security.acl package for J2SE 1.3</rdfs:comment>
		<rdfs:comment xml:lang="OWLManchester">platform:comprisesInterfacePart some JavaSecurityAcl</rdfs:comment>
	</owl:Class>
	<owl:Class rdf:about="#JavaUtilAPI">
		<rdfs:subClassOf rdf:resource="&j2me-pp-1_0;JavaUtilAPI"/>
		<rdfs:subClassOf rdf:resource="&j2se-1_2;JavaUtilAPI"/>
		<rdfs:comment xml:lang="en">JavaLibrary implementing the java.util package for J2SE 1.3</rdfs:comment>
		<rdfs:comment xml:lang="OWLManchester">platform:comprisesInterfacePart some JavaUtil</rdfs:comment>
	</owl:Class>
	<owl:Class rdf:about="#JavaUtilJarAPI">
		<owl:equivalentClass rdf:resource="&j2me-pp-1_0;JavaUtilJarAPI"/>
		<rdfs:subClassOf rdf:resource="&j2se-1_2;JavaUtilJarAPI"/>
		<rdfs:comment xml:lang="en">JavaLibrary implementing the java.util.jar package for J2SE 1.3</rdfs:comment>
		<rdfs:comment xml:lang="OWLManchester">platform:comprisesInterfacePart some JavaUtilJar</rdfs:comment>
	</owl:Class>
	<owl:Class rdf:about="#JavaUtilZipAPI">
		<owl:equivalentClass rdf:resource="&j2me-pp-1_0;JavaUtilZipAPI"/>
		<rdfs:subClassOf rdf:resource="&j2se-1_2;JavaUtilZipAPI"/>
		<rdfs:comment xml:lang="en">JavaLibrary implementing the java.util.zip package for J2SE 1.3</rdfs:comment>
		<rdfs:comment xml:lang="OWLManchester">platform:comprisesInterfacePart some JavaUtilZip</rdfs:comment>
	</owl:Class>
	<owl:Class rdf:about="#JavaMathAPI">
		<owl:equivalentClass rdf:resource="&j2me-pp-1_0;JavaMathAPI"/>
		<owl:equivalentClass rdf:resource="&j2se-1_2;JavaMathAPI"/>
		<rdfs:subClassOf rdf:resource="&java;JavaAPI"/>
		<rdfs:comment xml:lang="en">JavaLibrary implementing the java.math package for J2SE 1.3</rdfs:comment>
		<rdfs:comment xml:lang="OWLManchester">platform:comprisesInterfacePart some JavaMath</rdfs:comment>
	</owl:Class>
	<owl:Class rdf:about="#JavaTextAPI">
		<owl:equivalentClass rdf:resource="&j2me-pp-1_0;JavaTextAPI"/>
		<rdfs:subClassOf rdf:resource="&java;JavaAPI"/>
		<rdfs:comment xml:lang="en">JavaLibrary implementing the java.text package for J2SE 1.3</rdfs:comment>
		<rdfs:comment xml:lang="OWLManchester">platform:comprisesInterfacePart some JavaText</rdfs:comment>
	</owl:Class>
	<owl:Class rdf:about="#JavaTextResourcesAPI">
		<owl:equivalentClass rdf:resource="&j2me-pp-1_0;JavaTextResourcesAPI"/>
		<rdfs:subClassOf rdf:resource="&java;JavaAPI"/>
		<rdfs:comment xml:lang="en">JavaLibrary implementing the java.text.resources package for J2SE 1.3</rdfs:comment>
		<rdfs:comment xml:lang="OWLManchester">platform:comprisesInterfacePart some JavaTextResources</rdfs:comment>
	</owl:Class>
	<owl:Class rdf:about="#JavaAwtAPI">
		<rdfs:subClassOf rdf:resource="&j2me-pp-1_0;JavaAwtAPI"/>
		<rdfs:subClassOf rdf:resource="&j2se-1_2;JavaAwtAPI"/>
		<rdfs:comment xml:lang="en">JavaLibrary implementing the java.awt package for J2SE 1.3</rdfs:comment>
		<rdfs:comment xml:lang="OWLManchester">platform:comprisesInterfacePart some JavaAwt</rdfs:comment>
	</owl:Class>
	<owl:Class rdf:about="#JavaAwtGeomAPI">
		<rdfs:subClassOf rdf:resource="&j2se-1_2;JavaAwtGeomAPI"/>
		<rdfs:comment xml:lang="en">JavaLibrary implementing the java.awt.geom package for J2SE 1.3</rdfs:comment>
		<rdfs:comment xml:lang="OWLManchester">platform:comprisesInterfacePart some JavaAwtGeom</rdfs:comment>
	</owl:Class>
	<owl:Class rdf:about="#JavaAwtEventAPI">
		<rdfs:subClassOf rdf:resource="&j2me-pp-1_0;JavaAwtEventAPI"/>
		<rdfs:subClassOf rdf:resource="&j2se-1_2;JavaAwtEventAPI"/>
		<rdfs:comment xml:lang="en">JavaLibrary implementing the java.awt.event package for J2SE 1.3</rdfs:comment>
		<rdfs:comment xml:lang="OWLManchester">platform:comprisesInterfacePart some JavaAwtEvent</rdfs:comment>
	</owl:Class>
	<owl:Class rdf:about="#JavaAwtFontAPI">
		<rdfs:subClassOf rdf:resource="&java;JavaAPI"/>
		<rdfs:comment xml:lang="en">JavaLibrary implementing the java.awt.font package for J2SE 1.3</rdfs:comment>
		<rdfs:comment xml:lang="OWLManchester">platform:comprisesInterfacePart some JavaAwtFont</rdfs:comment>
	</owl:Class>
	<owl:Class rdf:about="#JavaAwtImageAPI">
		<rdfs:subClassOf rdf:resource="&j2me-pp-1_0;JavaAwtImageAPI"/>
		<rdfs:subClassOf rdf:resource="&j2se-1_2;JavaAwtImageAPI"/>
		<rdfs:comment xml:lang="en">JavaLibrary implementing the java.awt.image package for J2SE 1.3</rdfs:comment>
		<rdfs:comment xml:lang="OWLManchester">platform:comprisesInterfacePart some JavaAwtImage</rdfs:comment>
	</owl:Class>
	<owl:Class rdf:about="#JavaAwtImageRenderableAPI">
		<rdfs:subClassOf rdf:resource="&j2se-1_2;JavaAwtImageRenderableAPI"/>
		<rdfs:comment xml:lang="en">JavaLibrary implementing the java.awt.image.renderable package for J2SE 1.3</rdfs:comment>
		<rdfs:comment xml:lang="OWLManchester">platform:comprisesInterfacePart some JavaAwtImageRenderable</rdfs:comment>
	</owl:Class>
	<owl:Class rdf:about="#JavaAwtDndAPI">
		<owl:equivalentClass rdf:resource="&j2se-1_2;JavaAwtDndAPI"/>
		<rdfs:subClassOf rdf:resource="&java;JavaAPI"/>
		<rdfs:comment xml:lang="en">JavaLibrary implementing the java.awt.dnd package for J2SE 1.3</rdfs:comment>
		<rdfs:comment xml:lang="OWLManchester">platform:comprisesInterfacePart some JavaAwtDnd</rdfs:comment>
	</owl:Class>
	<owl:Class rdf:about="#JavaAwtImAPI">
		<rdfs:subClassOf rdf:resource="&j2se-1_2;JavaAwtImAPI"/>
		<rdfs:comment xml:lang="en">JavaLibrary implementing the java.awt.im package for J2SE 1.3</rdfs:comment>
		<rdfs:comment xml:lang="OWLManchester">platform:comprisesInterfacePart some JavaAwtIm</rdfs:comment>
	</owl:Class>
	<owl:Class rdf:about="#JavaAwtImSpiAPI">
		<rdfs:subClassOf rdf:resource="&java;JavaAPI"/>
		<rdfs:comment xml:lang="en">JavaLibrary implementing the java.awt.im.spi package for J2SE 1.3</rdfs:comment>
		<rdfs:comment xml:lang="OWLManchester">platform:comprisesInterfacePart some JavaAwtImSpi</rdfs:comment>
	</owl:Class>
	<owl:Class rdf:about="#JavaAwtColorAPI">
		<rdfs:subClassOf rdf:resource="&j2me-pp-1_0;JavaAwtColorAPI"/>
		<rdfs:subClassOf rdf:resource="&j2se-1_2;JavaAwtColorAPI"/>
		<rdfs:comment xml:lang="en">JavaLibrary implementing the java.awt.color package for J2SE 1.3</rdfs:comment>
		<rdfs:comment xml:lang="OWLManchester">platform:comprisesInterfacePart some JavaAwtColor</rdfs:comment>
	</owl:Class>
	<owl:Class rdf:about="#JavaAwtDatatransferAPI">
		<rdfs:subClassOf rdf:resource="&j2me-pp-1_0;JavaAwtDatatransferAPI"/>
		<rdfs:subClassOf rdf:resource="&j2se-1_2;JavaAwtDatatransferAPI"/>
		<rdfs:comment xml:lang="en">JavaLibrary implementing the java.awt.datatransfer package for J2SE 1.3</rdfs:comment>
		<rdfs:comment xml:lang="OWLManchester">platform:comprisesInterfacePart some JavaAwtDatatransfer</rdfs:comment>
	</owl:Class>
	<owl:Class rdf:about="#JavaAwtPrintAPI">
		<owl:equivalentClass rdf:resource="&j2se-1_2;JavaAwtPrintAPI"/>
		<rdfs:subClassOf rdf:resource="&java;JavaAPI"/>
		<rdfs:comment xml:lang="en">JavaLibrary implementing the java.awt.print package for J2SE 1.3</rdfs:comment>
		<rdfs:comment xml:lang="OWLManchester">platform:comprisesInterfacePart some JavaAwtPrint</rdfs:comment>
	</owl:Class>
	<owl:Class rdf:about="#JavaBeansAPI">
		<owl:equivalentClass rdf:resource="&j2se-1_2;JavaBeansAPI"/>
		<rdfs:subClassOf rdf:resource="&j2me-pp-1_0;JavaBeansAPI"/>
		<rdfs:comment xml:lang="en">JavaLibrary implementing the java.beans package for J2SE 1.3</rdfs:comment>
		<rdfs:comment xml:lang="OWLManchester">platform:comprisesInterfacePart some JavaBeans</rdfs:comment>
	</owl:Class>
	<owl:Class rdf:about="#JavaBeansBeancontextAPI">
		<owl:equivalentClass rdf:resource="&j2se-1_2;JavaBeansBeancontextAPI"/>
		<rdfs:subClassOf rdf:resource="&java;JavaAPI"/>
		<rdfs:comment xml:lang="en">JavaLibrary implementing the java.beans.beancontext package for J2SE 1.3</rdfs:comment>
		<rdfs:comment xml:lang="OWLManchester">platform:comprisesInterfacePart some JavaBeansBeancontext</rdfs:comment>
	</owl:Class>
	<owl:Class rdf:about="#JavaAppletAPI">
		<rdfs:subClassOf rdf:resource="&j2me-pp-1_0;JavaAppletAPI"/>
		<rdfs:subClassOf rdf:resource="&j2se-1_2;JavaAppletAPI"/>
		<rdfs:comment xml:lang="en">JavaLibrary implementing the java.applet package for J2SE 1.3</rdfs:comment>
		<rdfs:comment xml:lang="OWLManchester">platform:comprisesInterfacePart some JavaApplet</rdfs:comment>
	</owl:Class>
	<owl:Class rdf:about="#JavaRmiAPI">
		<owl:equivalentClass rdf:resource="&j2se-1_2;JavaRmiAPI"/>
		<rdfs:subClassOf rdf:resource="&j2me-pp-1_0;JavaRmiAPI"/>
		<rdfs:comment xml:lang="en">JavaLibrary implementing the java.rmi package for J2SE 1.3</rdfs:comment>
		<rdfs:comment xml:lang="OWLManchester">platform:comprisesInterfacePart some JavaRmi</rdfs:comment>
	</owl:Class>
	<owl:Class rdf:about="#JavaRmiServerAPI">
		<rdfs:subClassOf rdf:resource="&j2se-1_2;JavaRmiServerAPI"/>
		<rdfs:comment xml:lang="en">JavaLibrary implementing the java.rmi.server package for J2SE 1.3</rdfs:comment>
		<rdfs:comment xml:lang="OWLManchester">platform:comprisesInterfacePart some JavaRmiServer</rdfs:comment>
	</owl:Class>
	<owl:Class rdf:about="#JavaRmiDgcAPI">
		<owl:equivalentClass rdf:resource="&j2se-1_2;JavaRmiDgcAPI"/>
		<rdfs:subClassOf rdf:resource="&java;JavaAPI"/>
		<rdfs:comment xml:lang="en">JavaLibrary implementing the java.rmi.dgc package for J2SE 1.3</rdfs:comment>
		<rdfs:comment xml:lang="OWLManchester">platform:comprisesInterfacePart some JavaRmiDgc</rdfs:comment>
	</owl:Class>
	<owl:Class rdf:about="#JavaRmiRegistryAPI">
		<owl:equivalentClass rdf:resource="&j2se-1_2;JavaRmiRegistryAPI"/>
		<rdfs:subClassOf rdf:resource="&j2me-pp-1_0;JavaRmiRegistryAPI"/>
		<rdfs:comment xml:lang="en">JavaLibrary implementing the java.rmi.registry package for J2SE 1.3</rdfs:comment>
		<rdfs:comment xml:lang="OWLManchester">platform:comprisesInterfacePart some JavaRmiRegistry</rdfs:comment>
	</owl:Class>
	<owl:Class rdf:about="#JavaRmiActivationAPI">
		<owl:equivalentClass rdf:resource="&j2se-1_2;JavaRmiActivationAPI"/>
		<rdfs:subClassOf rdf:resource="&java;JavaAPI"/>
		<rdfs:comment xml:lang="en">JavaLibrary implementing the java.rmi.activation package for J2SE 1.3</rdfs:comment>
		<rdfs:comment xml:lang="OWLManchester">platform:comprisesInterfacePart some JavaRmiActivation</rdfs:comment>
	</owl:Class>
	<owl:Class rdf:about="#JavaSqlAPI">
		<rdfs:subClassOf rdf:resource="&j2se-1_2;JavaSqlAPI"/>
		<rdfs:comment xml:lang="en">JavaLibrary implementing the java.sql package for J2SE 1.3</rdfs:comment>
		<rdfs:comment xml:lang="OWLManchester">platform:comprisesInterfacePart some JavaSql</rdfs:comment>
	</owl:Class>
	<owl:Class rdf:about="#JavaxAccessibilityAPI">
		<rdfs:subClassOf rdf:resource="&j2se-1_2;JavaxAccessibilityAPI"/>
		<rdfs:comment xml:lang="en">JavaLibrary implementing the javax.accessibility package for J2SE 1.3</rdfs:comment>
		<rdfs:comment xml:lang="OWLManchester">platform:comprisesInterfacePart some JavaxAccessibility</rdfs:comment>
	</owl:Class>
	<owl:Class rdf:about="#JavaxSwingAPI">
		<rdfs:subClassOf rdf:resource="&java;JavaAPI"/>
		<rdfs:comment xml:lang="en">JavaLibrary implementing the javax.swing package for J2SE 1.3</rdfs:comment>
		<rdfs:comment xml:lang="OWLManchester">platform:comprisesInterfacePart some JavaxSwing</rdfs:comment>
	</owl:Class>
	<owl:Class rdf:about="#JavaxSwingTextAPI">
		<rdfs:subClassOf rdf:resource="&j2se-1_2;JavaxSwingTextAPI"/>
		<rdfs:comment xml:lang="en">JavaLibrary implementing the javax.swing.text package for J2SE 1.3</rdfs:comment>
		<rdfs:comment xml:lang="OWLManchester">platform:comprisesInterfacePart some JavaxSwingText</rdfs:comment>
	</owl:Class>
	<owl:Class rdf:about="#JavaxSwingTextHtmlAPI">
		<rdfs:subClassOf rdf:resource="&j2se-1_2;JavaxSwingTextHtmlAPI"/>
		<rdfs:comment xml:lang="en">JavaLibrary implementing the javax.swing.text.html package for J2SE 1.3</rdfs:comment>
		<rdfs:comment xml:lang="OWLManchester">platform:comprisesInterfacePart some JavaxSwingTextHtml</rdfs:comment>
	</owl:Class>
	<owl:Class rdf:about="#JavaxSwingTextHtmlParserAPI">
		<rdfs:subClassOf rdf:resource="&j2se-1_2;JavaxSwingTextHtmlParserAPI"/>
		<rdfs:comment xml:lang="en">JavaLibrary implementing the javax.swing.text.html.parser package for J2SE 1.3</rdfs:comment>
		<rdfs:comment xml:lang="OWLManchester">platform:comprisesInterfacePart some JavaxSwingTextHtmlParser</rdfs:comment>
	</owl:Class>
	<owl:Class rdf:about="#JavaxSwingTextRtfAPI">
		<owl:equivalentClass rdf:resource="&j2se-1_2;JavaxSwingTextRtfAPI"/>
		<rdfs:subClassOf rdf:resource="&java;JavaAPI"/>
		<rdfs:comment xml:lang="en">JavaLibrary implementing the javax.swing.text.rtf package for J2SE 1.3</rdfs:comment>
		<rdfs:comment xml:lang="OWLManchester">platform:comprisesInterfacePart some JavaxSwingTextRtf</rdfs:comment>
	</owl:Class>
	<owl:Class rdf:about="#JavaxSwingEventAPI">
		<rdfs:subClassOf rdf:resource="&j2se-1_2;JavaxSwingEventAPI"/>
		<rdfs:comment xml:lang="en">JavaLibrary implementing the javax.swing.event package for J2SE 1.3</rdfs:comment>
		<rdfs:comment xml:lang="OWLManchester">platform:comprisesInterfacePart some JavaxSwingEvent</rdfs:comment>
	</owl:Class>
	<owl:Class rdf:about="#JavaxSwingPlafAPI">
		<rdfs:subClassOf rdf:resource="&j2se-1_2;JavaxSwingPlafAPI"/>
		<rdfs:comment xml:lang="en">JavaLibrary implementing the javax.swing.plaf package for J2SE 1.3</rdfs:comment>
		<rdfs:comment xml:lang="OWLManchester">platform:comprisesInterfacePart some JavaxSwingPlaf</rdfs:comment>
	</owl:Class>
	<owl:Class rdf:about="#JavaxSwingPlafBasicAPI">
		<rdfs:subClassOf rdf:resource="&j2se-1_2;JavaxSwingPlafBasicAPI"/>
		<rdfs:comment xml:lang="en">JavaLibrary implementing the javax.swing.plaf.basic package for J2SE 1.3</rdfs:comment>
		<rdfs:comment xml:lang="OWLManchester">platform:comprisesInterfacePart some JavaxSwingPlafBasic</rdfs:comment>
	</owl:Class>
	<owl:Class rdf:about="#JavaxSwingPlafMetalAPI">
		<rdfs:subClassOf rdf:resource="&j2se-1_2;JavaxSwingPlafMetalAPI"/>
		<rdfs:comment xml:lang="en">JavaLibrary implementing the javax.swing.plaf.metal package for J2SE 1.3</rdfs:comment>
		<rdfs:comment xml:lang="OWLManchester">platform:comprisesInterfacePart some JavaxSwingPlafMetal</rdfs:comment>
	</owl:Class>
	<owl:Class rdf:about="#JavaxSwingPlafMultiAPI">
		<rdfs:subClassOf rdf:resource="&j2se-1_2;JavaxSwingPlafMultiAPI"/>
		<rdfs:comment xml:lang="en">JavaLibrary implementing the javax.swing.plaf.multi package for J2SE 1.3</rdfs:comment>
		<rdfs:comment xml:lang="OWLManchester">platform:comprisesInterfacePart some JavaxSwingPlafMulti</rdfs:comment>
	</owl:Class>
	<owl:Class rdf:about="#JavaxSwingUndoAPI">
		<owl:equivalentClass rdf:resource="&j2se-1_2;JavaxSwingUndoAPI"/>
		<rdfs:subClassOf rdf:resource="&java;JavaAPI"/>
		<rdfs:comment xml:lang="en">JavaLibrary implementing the javax.swing.undo package for J2SE 1.3</rdfs:comment>
		<rdfs:comment xml:lang="OWLManchester">platform:comprisesInterfacePart some JavaxSwingUndo</rdfs:comment>
	</owl:Class>
	<owl:Class rdf:about="#JavaxSwingTreeAPI">
		<rdfs:subClassOf rdf:resource="&j2se-1_2;JavaxSwingTreeAPI"/>
		<rdfs:comment xml:lang="en">JavaLibrary implementing the javax.swing.tree package for J2SE 1.3</rdfs:comment>
		<rdfs:comment xml:lang="OWLManchester">platform:comprisesInterfacePart some JavaxSwingTree</rdfs:comment>
	</owl:Class>
	<owl:Class rdf:about="#JavaxSwingTableAPI">
		<rdfs:subClassOf rdf:resource="&j2se-1_2;JavaxSwingTableAPI"/>
		<rdfs:comment xml:lang="en">JavaLibrary implementing the javax.swing.table package for J2SE 1.3</rdfs:comment>
		<rdfs:comment xml:lang="OWLManchester">platform:comprisesInterfacePart some JavaxSwingTable</rdfs:comment>
	</owl:Class>
	<owl:Class rdf:about="#JavaxSwingBorderAPI">
		<rdfs:subClassOf rdf:resource="&j2se-1_2;JavaxSwingBorderAPI"/>
		<rdfs:comment xml:lang="en">JavaLibrary implementing the javax.swing.border package for J2SE 1.3</rdfs:comment>
		<rdfs:comment xml:lang="OWLManchester">platform:comprisesInterfacePart some JavaxSwingBorder</rdfs:comment>
	</owl:Class>
	<owl:Class rdf:about="#JavaxSwingColorchooserAPI">
		<rdfs:subClassOf rdf:resource="&j2se-1_2;JavaxSwingColorchooserAPI"/>
		<rdfs:comment xml:lang="en">JavaLibrary implementing the javax.swing.colorchooser package for J2SE 1.3</rdfs:comment>
		<rdfs:comment xml:lang="OWLManchester">platform:comprisesInterfacePart some JavaxSwingColorchooser</rdfs:comment>
	</owl:Class>
	<owl:Class rdf:about="#JavaxSwingFilechooserAPI">
		<rdfs:subClassOf rdf:resource="&j2se-1_2;JavaxSwingFilechooserAPI"/>
		<rdfs:comment xml:lang="en">JavaLibrary implementing the javax.swing.filechooser package for J2SE 1.3</rdfs:comment>
		<rdfs:comment xml:lang="OWLManchester">platform:comprisesInterfacePart some JavaxSwingFilechooser</rdfs:comment>
	</owl:Class>
	<owl:Class rdf:about="#JavaxNamingAPI">
		<rdfs:subClassOf rdf:resource="&java;JavaAPI"/>
		<rdfs:comment xml:lang="en">JavaLibrary implementing the javax.naming package for J2SE 1.3</rdfs:comment>
		<rdfs:comment xml:lang="OWLManchester">platform:comprisesInterfacePart some JavaxNaming</rdfs:comment>
	</owl:Class>
	<owl:Class rdf:about="#JavaxNamingDirectoryAPI">
		<rdfs:subClassOf rdf:resource="&java;JavaAPI"/>
		<rdfs:comment xml:lang="en">JavaLibrary implementing the javax.naming.directory package for J2SE 1.3</rdfs:comment>
		<rdfs:comment xml:lang="OWLManchester">platform:comprisesInterfacePart some JavaxNamingDirectory</rdfs:comment>
	</owl:Class>
	<owl:Class rdf:about="#JavaxNamingEventAPI">
		<rdfs:subClassOf rdf:resource="&java;JavaAPI"/>
		<rdfs:comment xml:lang="en">JavaLibrary implementing the javax.naming.event package for J2SE 1.3</rdfs:comment>
		<rdfs:comment xml:lang="OWLManchester">platform:comprisesInterfacePart some JavaxNamingEvent</rdfs:comment>
	</owl:Class>
	<owl:Class rdf:about="#JavaxNamingLdapAPI">
		<rdfs:subClassOf rdf:resource="&java;JavaAPI"/>
		<rdfs:comment xml:lang="en">JavaLibrary implementing the javax.naming.ldap package for J2SE 1.3</rdfs:comment>
		<rdfs:comment xml:lang="OWLManchester">platform:comprisesInterfacePart some JavaxNamingLdap</rdfs:comment>
	</owl:Class>
	<owl:Class rdf:about="#JavaxNamingSpiAPI">
		<rdfs:subClassOf rdf:resource="&java;JavaAPI"/>
		<rdfs:comment xml:lang="en">JavaLibrary implementing the javax.naming.spi package for J2SE 1.3</rdfs:comment>
		<rdfs:comment xml:lang="OWLManchester">platform:comprisesInterfacePart some JavaxNamingSpi</rdfs:comment>
	</owl:Class>
	<owl:Class rdf:about="#JavaxSoundMidiAPI">
		<rdfs:subClassOf rdf:resource="&java;JavaAPI"/>
		<rdfs:comment xml:lang="en">JavaLibrary implementing the javax.sound.midi package for J2SE 1.3</rdfs:comment>
		<rdfs:comment xml:lang="OWLManchester">platform:comprisesInterfacePart some JavaxSoundMidi</rdfs:comment>
	</owl:Class>
	<owl:Class rdf:about="#JavaxSoundMidiSpiAPI">
		<rdfs:subClassOf rdf:resource="&java;JavaAPI"/>
		<rdfs:comment xml:lang="en">JavaLibrary implementing the javax.sound.midi.spi package for J2SE 1.3</rdfs:comment>
		<rdfs:comment xml:lang="OWLManchester">platform:comprisesInterfacePart some JavaxSoundMidiSpi</rdfs:comment>
	</owl:Class>
	<owl:Class rdf:about="#JavaxSoundSampledAPI">
		<rdfs:subClassOf rdf:resource="&java;JavaAPI"/>
		<rdfs:comment xml:lang="en">JavaLibrary implementing the javax.sound.sampled package for J2SE 1.3</rdfs:comment>
		<rdfs:comment xml:lang="OWLManchester">platform:comprisesInterfacePart some JavaxSoundSampled</rdfs:comment>
	</owl:Class>
	<owl:Class rdf:about="#JavaxSoundSampledSpiAPI">
		<rdfs:subClassOf rdf:resource="&java;JavaAPI"/>
		<rdfs:comment xml:lang="en">JavaLibrary implementing the javax.sound.sampled.spi package for J2SE 1.3</rdfs:comment>
		<rdfs:comment xml:lang="OWLManchester">platform:comprisesInterfacePart some JavaxSoundSampledSpi</rdfs:comment>
	</owl:Class>
	<owl:Class rdf:about="#JavaxRmiAPI">
		<rdfs:subClassOf rdf:resource="&java;JavaAPI"/>
		<rdfs:comment xml:lang="en">JavaLibrary implementing the javax.rmi package for J2SE 1.3</rdfs:comment>
		<rdfs:comment xml:lang="OWLManchester">platform:comprisesInterfacePart some JavaxRmi</rdfs:comment>
	</owl:Class>
	<owl:Class rdf:about="#JavaxRmiCORBAAPI">
		<rdfs:subClassOf rdf:resource="&java;JavaAPI"/>
		<rdfs:comment xml:lang="en">JavaLibrary implementing the javax.rmi.CORBA package for J2SE 1.3</rdfs:comment>
		<rdfs:comment xml:lang="OWLManchester">platform:comprisesInterfacePart some JavaxRmiCORBA</rdfs:comment>
	</owl:Class>
	<owl:Class rdf:about="#JavaxTransactionAPI">
		<rdfs:subClassOf rdf:resource="&java;JavaAPI"/>
		<rdfs:comment xml:lang="en">JavaLibrary implementing the javax.transaction package for J2SE 1.3</rdfs:comment>
		<rdfs:comment xml:lang="OWLManchester">platform:comprisesInterfacePart some JavaxTransaction</rdfs:comment>
	</owl:Class>
	<owl:Class rdf:about="#OrgOmgCORBA_2_3API">
		<rdfs:subClassOf rdf:resource="&java;JavaAPI"/>
		<rdfs:comment xml:lang="en">JavaLibrary implementing the org.omg.CORBA_2_3 package for J2SE 1.3</rdfs:comment>
		<rdfs:comment xml:lang="OWLManchester">platform:comprisesInterfacePart some OrgOmgCORBA_2_3</rdfs:comment>
	</owl:Class>
	<owl:Class rdf:about="#OrgOmgCORBA_2_3PortableAPI">
		<rdfs:subClassOf rdf:resource="&java;JavaAPI"/>
		<rdfs:comment xml:lang="en">JavaLibrary implementing the org.omg.CORBA_2_3.portable package for J2SE 1.3</rdfs:comment>
		<rdfs:comment xml:lang="OWLManchester">platform:comprisesInterfacePart some OrgOmgCORBA_2_3Portable</rdfs:comment>
	</owl:Class>
	<owl:Class rdf:about="#OrgOmgCORBAAPI">
		<rdfs:subClassOf rdf:resource="&j2se-1_2;OrgOmgCORBAAPI"/>
		<rdfs:comment xml:lang="en">JavaLibrary implementing the org.omg.CORBA package for J2SE 1.3</rdfs:comment>
		<rdfs:comment xml:lang="OWLManchester">platform:comprisesInterfacePart some OrgOmgCORBA</rdfs:comment>
	</owl:Class>
	<owl:Class rdf:about="#OrgOmgCORBAPortableAPI">
		<rdfs:subClassOf rdf:resource="&j2se-1_2;OrgOmgCORBAPortableAPI"/>
		<rdfs:comment xml:lang="en">JavaLibrary implementing the org.omg.CORBA.portable package for J2SE 1.3</rdfs:comment>
		<rdfs:comment xml:lang="OWLManchester">platform:comprisesInterfacePart some OrgOmgCORBAPortable</rdfs:comment>
	</owl:Class>
	<owl:Class rdf:about="#OrgOmgCORBATypeCodePackageAPI">
		<owl:equivalentClass rdf:resource="&j2se-1_2;OrgOmgCORBATypeCodePackageAPI"/>
		<rdfs:subClassOf rdf:resource="&java;JavaAPI"/>
		<rdfs:comment xml:lang="en">JavaLibrary implementing the org.omg.CORBA.TypeCodePackage package for J2SE 1.3</rdfs:comment>
		<rdfs:comment xml:lang="OWLManchester">platform:comprisesInterfacePart some OrgOmgCORBATypeCodePackage</rdfs:comment>
	</owl:Class>
	<owl:Class rdf:about="#OrgOmgCORBAORBPackageAPI">
		<owl:equivalentClass rdf:resource="&j2se-1_2;OrgOmgCORBAORBPackageAPI"/>
		<rdfs:subClassOf rdf:resource="&java;JavaAPI"/>
		<rdfs:comment xml:lang="en">JavaLibrary implementing the org.omg.CORBA.ORBPackage package for J2SE 1.3</rdfs:comment>
		<rdfs:comment xml:lang="OWLManchester">platform:comprisesInterfacePart some OrgOmgCORBAORBPackage</rdfs:comment>
	</owl:Class>
	<owl:Class rdf:about="#OrgOmgCORBADynAnyPackageAPI">
		<owl:equivalentClass rdf:resource="&j2se-1_2;OrgOmgCORBADynAnyPackageAPI"/>
		<rdfs:subClassOf rdf:resource="&java;JavaAPI"/>
		<rdfs:comment xml:lang="en">JavaLibrary implementing the org.omg.CORBA.DynAnyPackage package for J2SE 1.3</rdfs:comment>
		<rdfs:comment xml:lang="OWLManchester">platform:comprisesInterfacePart some OrgOmgCORBADynAnyPackage</rdfs:comment>
	</owl:Class>
	<owl:Class rdf:about="#OrgOmgSendingContextAPI">
		<rdfs:subClassOf rdf:resource="&java;JavaAPI"/>
		<rdfs:comment xml:lang="en">JavaLibrary implementing the org.omg.SendingContext package for J2SE 1.3</rdfs:comment>
		<rdfs:comment xml:lang="OWLManchester">platform:comprisesInterfacePart some OrgOmgSendingContext</rdfs:comment>
	</owl:Class>
	<owl:Class rdf:about="#OrgOmgCosNamingAPI">
		<rdfs:subClassOf rdf:resource="&j2se-1_2;OrgOmgCosNamingAPI"/>
		<rdfs:comment xml:lang="en">JavaLibrary implementing the org.omg.CosNaming package for J2SE 1.3</rdfs:comment>
		<rdfs:comment xml:lang="OWLManchester">platform:comprisesInterfacePart some OrgOmgCosNaming</rdfs:comment>
	</owl:Class>
	<owl:Class rdf:about="#OrgOmgCosNamingNamingContextPackageAPI">
		<owl:equivalentClass rdf:resource="&j2se-1_2;OrgOmgCosNamingNamingContextPackageAPI"/>
		<rdfs:subClassOf rdf:resource="&java;JavaAPI"/>
		<rdfs:comment xml:lang="en">JavaLibrary implementing the org.omg.CosNaming.NamingContextPackage package for J2SE 1.3</rdfs:comment>
		<rdfs:comment xml:lang="OWLManchester">platform:comprisesInterfacePart some OrgOmgCosNamingNamingContextPackage</rdfs:comment>
	</owl:Class>
	<owl:Class rdf:about="#OrgOmgStubJavaRmiAPI">
		<rdfs:subClassOf rdf:resource="&java;JavaAPI"/>
		<rdfs:comment xml:lang="en">JavaLibrary implementing the org.omg.stub.java.rmi package for J2SE 1.3</rdfs:comment>
		<rdfs:comment xml:lang="OWLManchester">platform:comprisesInterfacePart some OrgOmgStubJavaRmi</rdfs:comment>
	</owl:Class>
	<JavaIo rdf:about="#theJavaIoPart">
	</JavaIo>
	<JavaLang rdf:about="#theJavaLangPart">
	</JavaLang>
	<JavaLangReflect rdf:about="#theJavaLangReflectPart">
	</JavaLangReflect>
	<JavaLangRef rdf:about="#theJavaLangRefPart">
	</JavaLangRef>
	<JavaNet rdf:about="#theJavaNetPart">
	</JavaNet>
	<JavaSecurity rdf:about="#theJavaSecurityPart">
	</JavaSecurity>
	<JavaSecurityCert rdf:about="#theJavaSecurityCertPart">
	</JavaSecurityCert>
	<JavaSecuritySpec rdf:about="#theJavaSecuritySpecPart">
	</JavaSecuritySpec>
	<JavaSecurityInterfaces rdf:about="#theJavaSecurityInterfacesPart">
	</JavaSecurityInterfaces>
	<JavaSecurityAcl rdf:about="#theJavaSecurityAclPart">
	</JavaSecurityAcl>
	<JavaUtil rdf:about="#theJavaUtilPart">
	</JavaUtil>
	<JavaUtilJar rdf:about="#theJavaUtilJarPart">
	</JavaUtilJar>
	<JavaUtilZip rdf:about="#theJavaUtilZipPart">
	</JavaUtilZip>
	<JavaMath rdf:about="#theJavaMathPart">
	</JavaMath>
	<JavaText rdf:about="#theJavaTextPart">
	</JavaText>
	<JavaTextResources rdf:about="#theJavaTextResourcesPart">
	</JavaTextResources>
	<JavaAwt rdf:about="#theJavaAwtPart">
	</JavaAwt>
	<JavaAwtGeom rdf:about="#theJavaAwtGeomPart">
	</JavaAwtGeom>
	<JavaAwtEvent rdf:about="#theJavaAwtEventPart">
	</JavaAwtEvent>
	<JavaAwtFont rdf:about="#theJavaAwtFontPart">
	</JavaAwtFont>
	<JavaAwtImage rdf:about="#theJavaAwtImagePart">
	</JavaAwtImage>
	<JavaAwtImageRenderable rdf:about="#theJavaAwtImageRenderablePart">
	</JavaAwtImageRenderable>
	<JavaAwtDnd rdf:about="#theJavaAwtDndPart">
	</JavaAwtDnd>
	<JavaAwtIm rdf:about="#theJavaAwtImPart">
	</JavaAwtIm>
	<JavaAwtImSpi rdf:about="#theJavaAwtImSpiPart">
	</JavaAwtImSpi>
	<JavaAwtColor rdf:about="#theJavaAwtColorPart">
	</JavaAwtColor>
	<JavaAwtDatatransfer rdf:about="#theJavaAwtDatatransferPart">
	</JavaAwtDatatransfer>
	<JavaAwtPrint rdf:about="#theJavaAwtPrintPart">
	</JavaAwtPrint>
	<JavaBeans rdf:about="#theJavaBeansPart">
	</JavaBeans>
	<JavaBeansBeancontext rdf:about="#theJavaBeansBeancontextPart">
	</JavaBeansBeancontext>
	<JavaApplet rdf:about="#theJavaAppletPart">
	</JavaApplet>
	<JavaRmi rdf:about="#theJavaRmiPart">
	</JavaRmi>
	<JavaRmiServer rdf:about="#theJavaRmiServerPart">
	</JavaRmiServer>
	<JavaRmiDgc rdf:about="#theJavaRmiDgcPart">
	</JavaRmiDgc>
	<JavaRmiRegistry rdf:about="#theJavaRmiRegistryPart">
	</JavaRmiRegistry>
	<JavaRmiActivation rdf:about="#theJavaRmiActivationPart">
	</JavaRmiActivation>
	<JavaSql rdf:about="#theJavaSqlPart">
	</JavaSql>
	<JavaxAccessibility rdf:about="#theJavaxAccessibilityPart">
	</JavaxAccessibility>
	<JavaxSwing rdf:about="#theJavaxSwingPart">
	</JavaxSwing>
	<JavaxSwingText rdf:about="#theJavaxSwingTextPart">
	</JavaxSwingText>
	<JavaxSwingTextHtml rdf:about="#theJavaxSwingTextHtmlPart">
	</JavaxSwingTextHtml>
	<JavaxSwingTextHtmlParser rdf:about="#theJavaxSwingTextHtmlParserPart">
	</JavaxSwingTextHtmlParser>
	<JavaxSwingTextRtf rdf:about="#theJavaxSwingTextRtfPart">
	</JavaxSwingTextRtf>
	<JavaxSwingEvent rdf:about="#theJavaxSwingEventPart">
	</JavaxSwingEvent>
	<JavaxSwingPlaf rdf:about="#theJavaxSwingPlafPart">
	</JavaxSwingPlaf>
	<JavaxSwingPlafBasic rdf:about="#theJavaxSwingPlafBasicPart">
	</JavaxSwingPlafBasic>
	<JavaxSwingPlafMetal rdf:about="#theJavaxSwingPlafMetalPart">
	</JavaxSwingPlafMetal>
	<JavaxSwingPlafMulti rdf:about="#theJavaxSwingPlafMultiPart">
	</JavaxSwingPlafMulti>
	<JavaxSwingUndo rdf:about="#theJavaxSwingUndoPart">
	</JavaxSwingUndo>
	<JavaxSwingTree rdf:about="#theJavaxSwingTreePart">
	</JavaxSwingTree>
	<JavaxSwingTable rdf:about="#theJavaxSwingTablePart">
	</JavaxSwingTable>
	<JavaxSwingBorder rdf:about="#theJavaxSwingBorderPart">
	</JavaxSwingBorder>
	<JavaxSwingColorchooser rdf:about="#theJavaxSwingColorchooserPart">
	</JavaxSwingColorchooser>
	<JavaxSwingFilechooser rdf:about="#theJavaxSwingFilechooserPart">
	</JavaxSwingFilechooser>
	<JavaxNaming rdf:about="#theJavaxNamingPart">
	</JavaxNaming>
	<JavaxNamingDirectory rdf:about="#theJavaxNamingDirectoryPart">
	</JavaxNamingDirectory>
	<JavaxNamingEvent rdf:about="#theJavaxNamingEventPart">
	</JavaxNamingEvent>
	<JavaxNamingLdap rdf:about="#theJavaxNamingLdapPart">
	</JavaxNamingLdap>
	<JavaxNamingSpi rdf:about="#theJavaxNamingSpiPart">
	</JavaxNamingSpi>
	<JavaxSoundMidi rdf:about="#theJavaxSoundMidiPart">
	</JavaxSoundMidi>
	<JavaxSoundMidiSpi rdf:about="#theJavaxSoundMidiSpiPart">
	</JavaxSoundMidiSpi>
	<JavaxSoundSampled rdf:about="#theJavaxSoundSampledPart">
	</JavaxSoundSampled>
	<JavaxSoundSampledSpi rdf:about="#theJavaxSoundSampledSpiPart">
	</JavaxSoundSampledSpi>
	<JavaxRmi rdf:about="#theJavaxRmiPart">
	</JavaxRmi>
	<JavaxRmiCORBA rdf:about="#theJavaxRmiCORBAPart">
	</JavaxRmiCORBA>
	<JavaxTransaction rdf:about="#theJavaxTransactionPart">
	</JavaxTransaction>
	<OrgOmgCORBA_2_3 rdf:about="#theOrgOmgCORBA_2_3Part">
	</OrgOmgCORBA_2_3>
	<OrgOmgCORBA_2_3Portable rdf:about="#theOrgOmgCORBA_2_3PortablePart">
	</OrgOmgCORBA_2_3Portable>
	<OrgOmgCORBA rdf:about="#theOrgOmgCORBAPart">
	</OrgOmgCORBA>
	<OrgOmgCORBAPortable rdf:about="#theOrgOmgCORBAPortablePart">
	</OrgOmgCORBAPortable>
	<OrgOmgCORBATypeCodePackage rdf:about="#theOrgOmgCORBATypeCodePackagePart">
	</OrgOmgCORBATypeCodePackage>
	<OrgOmgCORBAORBPackage rdf:about="#theOrgOmgCORBAORBPackagePart">
	</OrgOmgCORBAORBPackage>
	<OrgOmgCORBADynAnyPackage rdf:about="#theOrgOmgCORBADynAnyPackagePart">
	</OrgOmgCORBADynAnyPackage>
	<OrgOmgSendingContext rdf:about="#theOrgOmgSendingContextPart">
	</OrgOmgSendingContext>
	<OrgOmgCosNaming rdf:about="#theOrgOmgCosNamingPart">
	</OrgOmgCosNaming>
	<OrgOmgCosNamingNamingContextPackage rdf:about="#theOrgOmgCosNamingNamingContextPackagePart">
	</OrgOmgCosNamingNamingContextPackage>
	<OrgOmgStubJavaRmi rdf:about="#theOrgOmgStubJavaRmiPart">
	</OrgOmgStubJavaRmi>
	<owl:Class rdf:about="#JavaIoClassLibrary">
		<rdfs:subClassOf rdf:resource="&j2me-pp-1_0;JavaIoClassLibrary"/>
		<rdfs:subClassOf rdf:resource="&j2se-1_2;JavaIoClassLibrary"/>
		<rdfs:comment xml:lang="en">JavaLibrary implementing the java.io package for J2SE 1.3</rdfs:comment>
		<rdfs:comment xml:lang="OWLManchester">platform:implementsInterface some JavaIoAPI</rdfs:comment>
	</owl:Class>
	<owl:Class rdf:about="#JavaLangClassLibrary">
		<rdfs:subClassOf rdf:resource="&j2me-pp-1_0;JavaLangClassLibrary"/>
		<rdfs:subClassOf rdf:resource="&j2se-1_2;JavaLangClassLibrary"/>
		<rdfs:comment xml:lang="en">JavaLibrary implementing the java.lang package for J2SE 1.3</rdfs:comment>
		<rdfs:comment xml:lang="OWLManchester">platform:implementsInterface some JavaLangAPI</rdfs:comment>
	</owl:Class>
	<owl:Class rdf:about="#JavaLangReflectClassLibrary">
		<owl:equivalentClass rdf:resource="&j2me-pp-1_0;JavaLangReflectClassLibrary"/>
		<rdfs:subClassOf rdf:resource="&j2se-1_2;JavaLangReflectClassLibrary"/>
		<rdfs:comment xml:lang="en">JavaLibrary implementing the java.lang.reflect package for J2SE 1.3</rdfs:comment>
		<rdfs:comment xml:lang="OWLManchester">platform:implementsInterface some JavaLangReflectAPI</rdfs:comment>
	</owl:Class>
	<owl:Class rdf:about="#JavaLangRefClassLibrary">
		<owl:equivalentClass rdf:resource="&j2me-pp-1_0;JavaLangRefClassLibrary"/>
		<owl:equivalentClass rdf:resource="&j2se-1_2;JavaLangRefClassLibrary"/>
		<rdfs:subClassOf rdf:resource="&java;JavaClassLibrary"/>
		<rdfs:comment xml:lang="en">JavaLibrary implementing the java.lang.ref package for J2SE 1.3</rdfs:comment>
		<rdfs:comment xml:lang="OWLManchester">platform:implementsInterface some JavaLangRefAPI</rdfs:comment>
	</owl:Class>
	<owl:Class rdf:about="#JavaNetClassLibrary">
		<rdfs:subClassOf rdf:resource="&j2me-pp-1_0;JavaNetClassLibrary"/>
		<rdfs:subClassOf rdf:resource="&j2se-1_2;JavaNetClassLibrary"/>
		<rdfs:comment xml:lang="en">JavaLibrary implementing the java.net package for J2SE 1.3</rdfs:comment>
		<rdfs:comment xml:lang="OWLManchester">platform:implementsInterface some JavaNetAPI</rdfs:comment>
	</owl:Class>
	<owl:Class rdf:about="#JavaSecurityClassLibrary">
		<rdfs:subClassOf rdf:resource="&j2me-pp-1_0;JavaSecurityClassLibrary"/>
		<rdfs:subClassOf rdf:resource="&j2se-1_2;JavaSecurityClassLibrary"/>
		<rdfs:comment xml:lang="en">JavaLibrary implementing the java.security package for J2SE 1.3</rdfs:comment>
		<rdfs:comment xml:lang="OWLManchester">platform:implementsInterface some JavaSecurityAPI</rdfs:comment>
	</owl:Class>
	<owl:Class rdf:about="#JavaSecurityCertClassLibrary">
		<owl:equivalentClass rdf:resource="&j2me-pp-1_0;JavaSecurityCertClassLibrary"/>
		<rdfs:subClassOf rdf:resource="&j2se-1_2;JavaSecurityCertClassLibrary"/>
		<rdfs:comment xml:lang="en">JavaLibrary implementing the java.security.cert package for J2SE 1.3</rdfs:comment>
		<rdfs:comment xml:lang="OWLManchester">platform:implementsInterface some JavaSecurityCertAPI</rdfs:comment>
	</owl:Class>
	<owl:Class rdf:about="#JavaSecuritySpecClassLibrary">
		<owl:equivalentClass rdf:resource="&j2me-pp-1_0;JavaSecuritySpecClassLibrary"/>
		<rdfs:subClassOf rdf:resource="&j2se-1_2;JavaSecuritySpecClassLibrary"/>
		<rdfs:comment xml:lang="en">JavaLibrary implementing the java.security.spec package for J2SE 1.3</rdfs:comment>
		<rdfs:comment xml:lang="OWLManchester">platform:implementsInterface some JavaSecuritySpecAPI</rdfs:comment>
	</owl:Class>
	<owl:Class rdf:about="#JavaSecurityInterfacesClassLibrary">
		<owl:equivalentClass rdf:resource="&j2me-pp-1_0;JavaSecurityInterfacesClassLibrary"/>
		<rdfs:subClassOf rdf:resource="&j2se-1_2;JavaSecurityInterfacesClassLibrary"/>
		<rdfs:comment xml:lang="en">JavaLibrary implementing the java.security.interfaces package for J2SE 1.3</rdfs:comment>
		<rdfs:comment xml:lang="OWLManchester">platform:implementsInterface some JavaSecurityInterfacesAPI</rdfs:comment>
	</owl:Class>
	<owl:Class rdf:about="#JavaSecurityAclClassLibrary">
		<owl:equivalentClass rdf:resource="&j2me-pp-1_0;JavaSecurityAclClassLibrary"/>
		<owl:equivalentClass rdf:resource="&j2se-1_2;JavaSecurityAclClassLibrary"/>
		<rdfs:subClassOf rdf:resource="&java;JavaClassLibrary"/>
		<rdfs:comment xml:lang="en">JavaLibrary implementing the java.security.acl package for J2SE 1.3</rdfs:comment>
		<rdfs:comment xml:lang="OWLManchester">platform:implementsInterface some JavaSecurityAclAPI</rdfs:comment>
	</owl:Class>
	<owl:Class rdf:about="#JavaUtilClassLibrary">
		<rdfs:subClassOf rdf:resource="&j2me-pp-1_0;JavaUtilClassLibrary"/>
		<rdfs:subClassOf rdf:resource="&j2se-1_2;JavaUtilClassLibrary"/>
		<rdfs:comment xml:lang="en">JavaLibrary implementing the java.util package for J2SE 1.3</rdfs:comment>
		<rdfs:comment xml:lang="OWLManchester">platform:implementsInterface some JavaUtilAPI</rdfs:comment>
	</owl:Class>
	<owl:Class rdf:about="#JavaUtilJarClassLibrary">
		<owl:equivalentClass rdf:resource="&j2me-pp-1_0;JavaUtilJarClassLibrary"/>
		<rdfs:subClassOf rdf:resource="&j2se-1_2;JavaUtilJarClassLibrary"/>
		<rdfs:comment xml:lang="en">JavaLibrary implementing the java.util.jar package for J2SE 1.3</rdfs:comment>
		<rdfs:comment xml:lang="OWLManchester">platform:implementsInterface some JavaUtilJarAPI</rdfs:comment>
	</owl:Class>
	<owl:Class rdf:about="#JavaUtilZipClassLibrary">
		<owl:equivalentClass rdf:resource="&j2me-pp-1_0;JavaUtilZipClassLibrary"/>
		<rdfs:subClassOf rdf:resource="&j2se-1_2;JavaUtilZipClassLibrary"/>
		<rdfs:comment xml:lang="en">JavaLibrary implementing the java.util.zip package for J2SE 1.3</rdfs:comment>
		<rdfs:comment xml:lang="OWLManchester">platform:implementsInterface some JavaUtilZipAPI</rdfs:comment>
	</owl:Class>
	<owl:Class rdf:about="#JavaMathClassLibrary">
		<owl:equivalentClass rdf:resource="&j2me-pp-1_0;JavaMathClassLibrary"/>
		<owl:equivalentClass rdf:resource="&j2se-1_2;JavaMathClassLibrary"/>
		<rdfs:subClassOf rdf:resource="&java;JavaClassLibrary"/>
		<rdfs:comment xml:lang="en">JavaLibrary implementing the java.math package for J2SE 1.3</rdfs:comment>
		<rdfs:comment xml:lang="OWLManchester">platform:implementsInterface some JavaMathAPI</rdfs:comment>
	</owl:Class>
	<owl:Class rdf:about="#JavaTextClassLibrary">
		<owl:equivalentClass rdf:resource="&j2me-pp-1_0;JavaTextClassLibrary"/>
		<rdfs:subClassOf rdf:resource="&java;JavaClassLibrary"/>
		<rdfs:comment xml:lang="en">JavaLibrary implementing the java.text package for J2SE 1.3</rdfs:comment>
		<rdfs:comment xml:lang="OWLManchester">platform:implementsInterface some JavaTextAPI</rdfs:comment>
	</owl:Class>
	<owl:Class rdf:about="#JavaTextResourcesClassLibrary">
		<owl:equivalentClass rdf:resource="&j2me-pp-1_0;JavaTextResourcesClassLibrary"/>
		<rdfs:subClassOf rdf:resource="&java;JavaClassLibrary"/>
		<rdfs:comment xml:lang="en">JavaLibrary implementing the java.text.resources package for J2SE 1.3</rdfs:comment>
		<rdfs:comment xml:lang="OWLManchester">platform:implementsInterface some JavaTextResourcesAPI</rdfs:comment>
	</owl:Class>
	<owl:Class rdf:about="#JavaAwtClassLibrary">
		<rdfs:subClassOf rdf:resource="&j2me-pp-1_0;JavaAwtClassLibrary"/>
		<rdfs:subClassOf rdf:resource="&j2se-1_2;JavaAwtClassLibrary"/>
		<rdfs:comment xml:lang="en">JavaLibrary implementing the java.awt package for J2SE 1.3</rdfs:comment>
		<rdfs:comment xml:lang="OWLManchester">platform:implementsInterface some JavaAwtAPI</rdfs:comment>
	</owl:Class>
	<owl:Class rdf:about="#JavaAwtGeomClassLibrary">
		<rdfs:subClassOf rdf:resource="&j2se-1_2;JavaAwtGeomClassLibrary"/>
		<rdfs:comment xml:lang="en">JavaLibrary implementing the java.awt.geom package for J2SE 1.3</rdfs:comment>
		<rdfs:comment xml:lang="OWLManchester">platform:implementsInterface some JavaAwtGeomAPI</rdfs:comment>
	</owl:Class>
	<owl:Class rdf:about="#JavaAwtEventClassLibrary">
		<rdfs:subClassOf rdf:resource="&j2me-pp-1_0;JavaAwtEventClassLibrary"/>
		<rdfs:subClassOf rdf:resource="&j2se-1_2;JavaAwtEventClassLibrary"/>
		<rdfs:comment xml:lang="en">JavaLibrary implementing the java.awt.event package for J2SE 1.3</rdfs:comment>
		<rdfs:comment xml:lang="OWLManchester">platform:implementsInterface some JavaAwtEventAPI</rdfs:comment>
	</owl:Class>
	<owl:Class rdf:about="#JavaAwtFontClassLibrary">
		<rdfs:subClassOf rdf:resource="&java;JavaClassLibrary"/>
		<rdfs:comment xml:lang="en">JavaLibrary implementing the java.awt.font package for J2SE 1.3</rdfs:comment>
		<rdfs:comment xml:lang="OWLManchester">platform:implementsInterface some JavaAwtFontAPI</rdfs:comment>
	</owl:Class>
	<owl:Class rdf:about="#JavaAwtImageClassLibrary">
		<rdfs:subClassOf rdf:resource="&j2me-pp-1_0;JavaAwtImageClassLibrary"/>
		<rdfs:subClassOf rdf:resource="&j2se-1_2;JavaAwtImageClassLibrary"/>
		<rdfs:comment xml:lang="en">JavaLibrary implementing the java.awt.image package for J2SE 1.3</rdfs:comment>
		<rdfs:comment xml:lang="OWLManchester">platform:implementsInterface some JavaAwtImageAPI</rdfs:comment>
	</owl:Class>
	<owl:Class rdf:about="#JavaAwtImageRenderableClassLibrary">
		<rdfs:subClassOf rdf:resource="&j2se-1_2;JavaAwtImageRenderableClassLibrary"/>
		<rdfs:comment xml:lang="en">JavaLibrary implementing the java.awt.image.renderable package for J2SE 1.3</rdfs:comment>
		<rdfs:comment xml:lang="OWLManchester">platform:implementsInterface some JavaAwtImageRenderableAPI</rdfs:comment>
	</owl:Class>
	<owl:Class rdf:about="#JavaAwtDndClassLibrary">
		<owl:equivalentClass rdf:resource="&j2se-1_2;JavaAwtDndClassLibrary"/>
		<rdfs:subClassOf rdf:resource="&java;JavaClassLibrary"/>
		<rdfs:comment xml:lang="en">JavaLibrary implementing the java.awt.dnd package for J2SE 1.3</rdfs:comment>
		<rdfs:comment xml:lang="OWLManchester">platform:implementsInterface some JavaAwtDndAPI</rdfs:comment>
	</owl:Class>
	<owl:Class rdf:about="#JavaAwtImClassLibrary">
		<rdfs:subClassOf rdf:resource="&j2se-1_2;JavaAwtImClassLibrary"/>
		<rdfs:comment xml:lang="en">JavaLibrary implementing the java.awt.im package for J2SE 1.3</rdfs:comment>
		<rdfs:comment xml:lang="OWLManchester">platform:implementsInterface some JavaAwtImAPI</rdfs:comment>
	</owl:Class>
	<owl:Class rdf:about="#JavaAwtImSpiClassLibrary">
		<rdfs:subClassOf rdf:resource="&java;JavaClassLibrary"/>
		<rdfs:comment xml:lang="en">JavaLibrary implementing the java.awt.im.spi package for J2SE 1.3</rdfs:comment>
		<rdfs:comment xml:lang="OWLManchester">platform:implementsInterface some JavaAwtImSpiAPI</rdfs:comment>
	</owl:Class>
	<owl:Class rdf:about="#JavaAwtColorClassLibrary">
		<rdfs:subClassOf rdf:resource="&j2me-pp-1_0;JavaAwtColorClassLibrary"/>
		<rdfs:subClassOf rdf:resource="&j2se-1_2;JavaAwtColorClassLibrary"/>
		<rdfs:comment xml:lang="en">JavaLibrary implementing the java.awt.color package for J2SE 1.3</rdfs:comment>
		<rdfs:comment xml:lang="OWLManchester">platform:implementsInterface some JavaAwtColorAPI</rdfs:comment>
	</owl:Class>
	<owl:Class rdf:about="#JavaAwtDatatransferClassLibrary">
		<rdfs:subClassOf rdf:resource="&j2me-pp-1_0;JavaAwtDatatransferClassLibrary"/>
		<rdfs:subClassOf rdf:resource="&j2se-1_2;JavaAwtDatatransferClassLibrary"/>
		<rdfs:comment xml:lang="en">JavaLibrary implementing the java.awt.datatransfer package for J2SE 1.3</rdfs:comment>
		<rdfs:comment xml:lang="OWLManchester">platform:implementsInterface some JavaAwtDatatransferAPI</rdfs:comment>
	</owl:Class>
	<owl:Class rdf:about="#JavaAwtPrintClassLibrary">
		<owl:equivalentClass rdf:resource="&j2se-1_2;JavaAwtPrintClassLibrary"/>
		<rdfs:subClassOf rdf:resource="&java;JavaClassLibrary"/>
		<rdfs:comment xml:lang="en">JavaLibrary implementing the java.awt.print package for J2SE 1.3</rdfs:comment>
		<rdfs:comment xml:lang="OWLManchester">platform:implementsInterface some JavaAwtPrintAPI</rdfs:comment>
	</owl:Class>
	<owl:Class rdf:about="#JavaBeansClassLibrary">
		<owl:equivalentClass rdf:resource="&j2se-1_2;JavaBeansClassLibrary"/>
		<rdfs:subClassOf rdf:resource="&j2me-pp-1_0;JavaBeansClassLibrary"/>
		<rdfs:comment xml:lang="en">JavaLibrary implementing the java.beans package for J2SE 1.3</rdfs:comment>
		<rdfs:comment xml:lang="OWLManchester">platform:implementsInterface some JavaBeansAPI</rdfs:comment>
	</owl:Class>
	<owl:Class rdf:about="#JavaBeansBeancontextClassLibrary">
		<owl:equivalentClass rdf:resource="&j2se-1_2;JavaBeansBeancontextClassLibrary"/>
		<rdfs:subClassOf rdf:resource="&java;JavaClassLibrary"/>
		<rdfs:comment xml:lang="en">JavaLibrary implementing the java.beans.beancontext package for J2SE 1.3</rdfs:comment>
		<rdfs:comment xml:lang="OWLManchester">platform:implementsInterface some JavaBeansBeancontextAPI</rdfs:comment>
	</owl:Class>
	<owl:Class rdf:about="#JavaAppletClassLibrary">
		<rdfs:subClassOf rdf:resource="&j2me-pp-1_0;JavaAppletClassLibrary"/>
		<rdfs:subClassOf rdf:resource="&j2se-1_2;JavaAppletClassLibrary"/>
		<rdfs:comment xml:lang="en">JavaLibrary implementing the java.applet package for J2SE 1.3</rdfs:comment>
		<rdfs:comment xml:lang="OWLManchester">platform:implementsInterface some JavaAppletAPI</rdfs:comment>
	</owl:Class>
	<owl:Class rdf:about="#JavaRmiClassLibrary">
		<owl:equivalentClass rdf:resource="&j2se-1_2;JavaRmiClassLibrary"/>
		<rdfs:subClassOf rdf:resource="&j2me-pp-1_0;JavaRmiClassLibrary"/>
		<rdfs:comment xml:lang="en">JavaLibrary implementing the java.rmi package for J2SE 1.3</rdfs:comment>
		<rdfs:comment xml:lang="OWLManchester">platform:implementsInterface some JavaRmiAPI</rdfs:comment>
	</owl:Class>
	<owl:Class rdf:about="#JavaRmiServerClassLibrary">
		<rdfs:subClassOf rdf:resource="&j2se-1_2;JavaRmiServerClassLibrary"/>
		<rdfs:comment xml:lang="en">JavaLibrary implementing the java.rmi.server package for J2SE 1.3</rdfs:comment>
		<rdfs:comment xml:lang="OWLManchester">platform:implementsInterface some JavaRmiServerAPI</rdfs:comment>
	</owl:Class>
	<owl:Class rdf:about="#JavaRmiDgcClassLibrary">
		<owl:equivalentClass rdf:resource="&j2se-1_2;JavaRmiDgcClassLibrary"/>
		<rdfs:subClassOf rdf:resource="&java;JavaClassLibrary"/>
		<rdfs:comment xml:lang="en">JavaLibrary implementing the java.rmi.dgc package for J2SE 1.3</rdfs:comment>
		<rdfs:comment xml:lang="OWLManchester">platform:implementsInterface some JavaRmiDgcAPI</rdfs:comment>
	</owl:Class>
	<owl:Class rdf:about="#JavaRmiRegistryClassLibrary">
		<owl:equivalentClass rdf:resource="&j2se-1_2;JavaRmiRegistryClassLibrary"/>
		<rdfs:subClassOf rdf:resource="&j2me-pp-1_0;JavaRmiRegistryClassLibrary"/>
		<rdfs:comment xml:lang="en">JavaLibrary implementing the java.rmi.registry package for J2SE 1.3</rdfs:comment>
		<rdfs:comment xml:lang="OWLManchester">platform:implementsInterface some JavaRmiRegistryAPI</rdfs:comment>
	</owl:Class>
	<owl:Class rdf:about="#JavaRmiActivationClassLibrary">
		<owl:equivalentClass rdf:resource="&j2se-1_2;JavaRmiActivationClassLibrary"/>
		<rdfs:subClassOf rdf:resource="&java;JavaClassLibrary"/>
		<rdfs:comment xml:lang="en">JavaLibrary implementing the java.rmi.activation package for J2SE 1.3</rdfs:comment>
		<rdfs:comment xml:lang="OWLManchester">platform:implementsInterface some JavaRmiActivationAPI</rdfs:comment>
	</owl:Class>
	<owl:Class rdf:about="#JavaSqlClassLibrary">
		<rdfs:subClassOf rdf:resource="&j2se-1_2;JavaSqlClassLibrary"/>
		<rdfs:comment xml:lang="en">JavaLibrary implementing the java.sql package for J2SE 1.3</rdfs:comment>
		<rdfs:comment xml:lang="OWLManchester">platform:implementsInterface some JavaSqlAPI</rdfs:comment>
	</owl:Class>
	<owl:Class rdf:about="#JavaxAccessibilityClassLibrary">
		<rdfs:subClassOf rdf:resource="&j2se-1_2;JavaxAccessibilityClassLibrary"/>
		<rdfs:comment xml:lang="en">JavaLibrary implementing the javax.accessibility package for J2SE 1.3</rdfs:comment>
		<rdfs:comment xml:lang="OWLManchester">platform:implementsInterface some JavaxAccessibilityAPI</rdfs:comment>
	</owl:Class>
	<owl:Class rdf:about="#JavaxSwingClassLibrary">
		<rdfs:subClassOf rdf:resource="&java;JavaClassLibrary"/>
		<rdfs:comment xml:lang="en">JavaLibrary implementing the javax.swing package for J2SE 1.3</rdfs:comment>
		<rdfs:comment xml:lang="OWLManchester">platform:implementsInterface some JavaxSwingAPI</rdfs:comment>
	</owl:Class>
	<owl:Class rdf:about="#JavaxSwingTextClassLibrary">
		<rdfs:subClassOf rdf:resource="&j2se-1_2;JavaxSwingTextClassLibrary"/>
		<rdfs:comment xml:lang="en">JavaLibrary implementing the javax.swing.text package for J2SE 1.3</rdfs:comment>
		<rdfs:comment xml:lang="OWLManchester">platform:implementsInterface some JavaxSwingTextAPI</rdfs:comment>
	</owl:Class>
	<owl:Class rdf:about="#JavaxSwingTextHtmlClassLibrary">
		<rdfs:subClassOf rdf:resource="&j2se-1_2;JavaxSwingTextHtmlClassLibrary"/>
		<rdfs:comment xml:lang="en">JavaLibrary implementing the javax.swing.text.html package for J2SE 1.3</rdfs:comment>
		<rdfs:comment xml:lang="OWLManchester">platform:implementsInterface some JavaxSwingTextHtmlAPI</rdfs:comment>
	</owl:Class>
	<owl:Class rdf:about="#JavaxSwingTextHtmlParserClassLibrary">
		<rdfs:subClassOf rdf:resource="&j2se-1_2;JavaxSwingTextHtmlParserClassLibrary"/>
		<rdfs:comment xml:lang="en">JavaLibrary implementing the javax.swing.text.html.parser package for J2SE 1.3</rdfs:comment>
		<rdfs:comment xml:lang="OWLManchester">platform:implementsInterface some JavaxSwingTextHtmlParserAPI</rdfs:comment>
	</owl:Class>
	<owl:Class rdf:about="#JavaxSwingTextRtfClassLibrary">
		<owl:equivalentClass rdf:resource="&j2se-1_2;JavaxSwingTextRtfClassLibrary"/>
		<rdfs:subClassOf rdf:resource="&java;JavaClassLibrary"/>
		<rdfs:comment xml:lang="en">JavaLibrary implementing the javax.swing.text.rtf package for J2SE 1.3</rdfs:comment>
		<rdfs:comment xml:lang="OWLManchester">platform:implementsInterface some JavaxSwingTextRtfAPI</rdfs:comment>
	</owl:Class>
	<owl:Class rdf:about="#JavaxSwingEventClassLibrary">
		<rdfs:subClassOf rdf:resource="&j2se-1_2;JavaxSwingEventClassLibrary"/>
		<rdfs:comment xml:lang="en">JavaLibrary implementing the javax.swing.event package for J2SE 1.3</rdfs:comment>
		<rdfs:comment xml:lang="OWLManchester">platform:implementsInterface some JavaxSwingEventAPI</rdfs:comment>
	</owl:Class>
	<owl:Class rdf:about="#JavaxSwingPlafClassLibrary">
		<rdfs:subClassOf rdf:resource="&j2se-1_2;JavaxSwingPlafClassLibrary"/>
		<rdfs:comment xml:lang="en">JavaLibrary implementing the javax.swing.plaf package for J2SE 1.3</rdfs:comment>
		<rdfs:comment xml:lang="OWLManchester">platform:implementsInterface some JavaxSwingPlafAPI</rdfs:comment>
	</owl:Class>
	<owl:Class rdf:about="#JavaxSwingPlafBasicClassLibrary">
		<rdfs:subClassOf rdf:resource="&j2se-1_2;JavaxSwingPlafBasicClassLibrary"/>
		<rdfs:comment xml:lang="en">JavaLibrary implementing the javax.swing.plaf.basic package for J2SE 1.3</rdfs:comment>
		<rdfs:comment xml:lang="OWLManchester">platform:implementsInterface some JavaxSwingPlafBasicAPI</rdfs:comment>
	</owl:Class>
	<owl:Class rdf:about="#JavaxSwingPlafMetalClassLibrary">
		<rdfs:subClassOf rdf:resource="&j2se-1_2;JavaxSwingPlafMetalClassLibrary"/>
		<rdfs:comment xml:lang="en">JavaLibrary implementing the javax.swing.plaf.metal package for J2SE 1.3</rdfs:comment>
		<rdfs:comment xml:lang="OWLManchester">platform:implementsInterface some JavaxSwingPlafMetalAPI</rdfs:comment>
	</owl:Class>
	<owl:Class rdf:about="#JavaxSwingPlafMultiClassLibrary">
		<rdfs:subClassOf rdf:resource="&j2se-1_2;JavaxSwingPlafMultiClassLibrary"/>
		<rdfs:comment xml:lang="en">JavaLibrary implementing the javax.swing.plaf.multi package for J2SE 1.3</rdfs:comment>
		<rdfs:comment xml:lang="OWLManchester">platform:implementsInterface some JavaxSwingPlafMultiAPI</rdfs:comment>
	</owl:Class>
	<owl:Class rdf:about="#JavaxSwingUndoClassLibrary">
		<owl:equivalentClass rdf:resource="&j2se-1_2;JavaxSwingUndoClassLibrary"/>
		<rdfs:subClassOf rdf:resource="&java;JavaClassLibrary"/>
		<rdfs:comment xml:lang="en">JavaLibrary implementing the javax.swing.undo package for J2SE 1.3</rdfs:comment>
		<rdfs:comment xml:lang="OWLManchester">platform:implementsInterface some JavaxSwingUndoAPI</rdfs:comment>
	</owl:Class>
	<owl:Class rdf:about="#JavaxSwingTreeClassLibrary">
		<rdfs:subClassOf rdf:resource="&j2se-1_2;JavaxSwingTreeClassLibrary"/>
		<rdfs:comment xml:lang="en">JavaLibrary implementing the javax.swing.tree package for J2SE 1.3</rdfs:comment>
		<rdfs:comment xml:lang="OWLManchester">platform:implementsInterface some JavaxSwingTreeAPI</rdfs:comment>
	</owl:Class>
	<owl:Class rdf:about="#JavaxSwingTableClassLibrary">
		<rdfs:subClassOf rdf:resource="&j2se-1_2;JavaxSwingTableClassLibrary"/>
		<rdfs:comment xml:lang="en">JavaLibrary implementing the javax.swing.table package for J2SE 1.3</rdfs:comment>
		<rdfs:comment xml:lang="OWLManchester">platform:implementsInterface some JavaxSwingTableAPI</rdfs:comment>
	</owl:Class>
	<owl:Class rdf:about="#JavaxSwingBorderClassLibrary">
		<rdfs:subClassOf rdf:resource="&j2se-1_2;JavaxSwingBorderClassLibrary"/>
		<rdfs:comment xml:lang="en">JavaLibrary implementing the javax.swing.border package for J2SE 1.3</rdfs:comment>
		<rdfs:comment xml:lang="OWLManchester">platform:implementsInterface some JavaxSwingBorderAPI</rdfs:comment>
	</owl:Class>
	<owl:Class rdf:about="#JavaxSwingColorchooserClassLibrary">
		<rdfs:subClassOf rdf:resource="&j2se-1_2;JavaxSwingColorchooserClassLibrary"/>
		<rdfs:comment xml:lang="en">JavaLibrary implementing the javax.swing.colorchooser package for J2SE 1.3</rdfs:comment>
		<rdfs:comment xml:lang="OWLManchester">platform:implementsInterface some JavaxSwingColorchooserAPI</rdfs:comment>
	</owl:Class>
	<owl:Class rdf:about="#JavaxSwingFilechooserClassLibrary">
		<rdfs:subClassOf rdf:resource="&j2se-1_2;JavaxSwingFilechooserClassLibrary"/>
		<rdfs:comment xml:lang="en">JavaLibrary implementing the javax.swing.filechooser package for J2SE 1.3</rdfs:comment>
		<rdfs:comment xml:lang="OWLManchester">platform:implementsInterface some JavaxSwingFilechooserAPI</rdfs:comment>
	</owl:Class>
	<owl:Class rdf:about="#JavaxNamingClassLibrary">
		<rdfs:subClassOf rdf:resource="&java;JavaClassLibrary"/>
		<rdfs:comment xml:lang="en">JavaLibrary implementing the javax.naming package for J2SE 1.3</rdfs:comment>
		<rdfs:comment xml:lang="OWLManchester">platform:implementsInterface some JavaxNamingAPI</rdfs:comment>
	</owl:Class>
	<owl:Class rdf:about="#JavaxNamingDirectoryClassLibrary">
		<rdfs:subClassOf rdf:resource="&java;JavaClassLibrary"/>
		<rdfs:comment xml:lang="en">JavaLibrary implementing the javax.naming.directory package for J2SE 1.3</rdfs:comment>
		<rdfs:comment xml:lang="OWLManchester">platform:implementsInterface some JavaxNamingDirectoryAPI</rdfs:comment>
	</owl:Class>
	<owl:Class rdf:about="#JavaxNamingEventClassLibrary">
		<rdfs:subClassOf rdf:resource="&java;JavaClassLibrary"/>
		<rdfs:comment xml:lang="en">JavaLibrary implementing the javax.naming.event package for J2SE 1.3</rdfs:comment>
		<rdfs:comment xml:lang="OWLManchester">platform:implementsInterface some JavaxNamingEventAPI</rdfs:comment>
	</owl:Class>
	<owl:Class rdf:about="#JavaxNamingLdapClassLibrary">
		<rdfs:subClassOf rdf:resource="&java;JavaClassLibrary"/>
		<rdfs:comment xml:lang="en">JavaLibrary implementing the javax.naming.ldap package for J2SE 1.3</rdfs:comment>
		<rdfs:comment xml:lang="OWLManchester">platform:implementsInterface some JavaxNamingLdapAPI</rdfs:comment>
	</owl:Class>
	<owl:Class rdf:about="#JavaxNamingSpiClassLibrary">
		<rdfs:subClassOf rdf:resource="&java;JavaClassLibrary"/>
		<rdfs:comment xml:lang="en">JavaLibrary implementing the javax.naming.spi package for J2SE 1.3</rdfs:comment>
		<rdfs:comment xml:lang="OWLManchester">platform:implementsInterface some JavaxNamingSpiAPI</rdfs:comment>
	</owl:Class>
	<owl:Class rdf:about="#JavaxSoundMidiClassLibrary">
		<rdfs:subClassOf rdf:resource="&java;JavaClassLibrary"/>
		<rdfs:comment xml:lang="en">JavaLibrary implementing the javax.sound.midi package for J2SE 1.3</rdfs:comment>
		<rdfs:comment xml:lang="OWLManchester">platform:implementsInterface some JavaxSoundMidiAPI</rdfs:comment>
	</owl:Class>
	<owl:Class rdf:about="#JavaxSoundMidiSpiClassLibrary">
		<rdfs:subClassOf rdf:resource="&java;JavaClassLibrary"/>
		<rdfs:comment xml:lang="en">JavaLibrary implementing the javax.sound.midi.spi package for J2SE 1.3</rdfs:comment>
		<rdfs:comment xml:lang="OWLManchester">platform:implementsInterface some JavaxSoundMidiSpiAPI</rdfs:comment>
	</owl:Class>
	<owl:Class rdf:about="#JavaxSoundSampledClassLibrary">
		<rdfs:subClassOf rdf:resource="&java;JavaClassLibrary"/>
		<rdfs:comment xml:lang="en">JavaLibrary implementing the javax.sound.sampled package for J2SE 1.3</rdfs:comment>
		<rdfs:comment xml:lang="OWLManchester">platform:implementsInterface some JavaxSoundSampledAPI</rdfs:comment>
	</owl:Class>
	<owl:Class rdf:about="#JavaxSoundSampledSpiClassLibrary">
		<rdfs:subClassOf rdf:resource="&java;JavaClassLibrary"/>
		<rdfs:comment xml:lang="en">JavaLibrary implementing the javax.sound.sampled.spi package for J2SE 1.3</rdfs:comment>
		<rdfs:comment xml:lang="OWLManchester">platform:implementsInterface some JavaxSoundSampledSpiAPI</rdfs:comment>
	</owl:Class>
	<owl:Class rdf:about="#JavaxRmiClassLibrary">
		<rdfs:subClassOf rdf:resource="&java;JavaClassLibrary"/>
		<rdfs:comment xml:lang="en">JavaLibrary implementing the javax.rmi package for J2SE 1.3</rdfs:comment>
		<rdfs:comment xml:lang="OWLManchester">platform:implementsInterface some JavaxRmiAPI</rdfs:comment>
	</owl:Class>
	<owl:Class rdf:about="#JavaxRmiCORBAClassLibrary">
		<rdfs:subClassOf rdf:resource="&java;JavaClassLibrary"/>
		<rdfs:comment xml:lang="en">JavaLibrary implementing the javax.rmi.CORBA package for J2SE 1.3</rdfs:comment>
		<rdfs:comment xml:lang="OWLManchester">platform:implementsInterface some JavaxRmiCORBAAPI</rdfs:comment>
	</owl:Class>
	<owl:Class rdf:about="#JavaxTransactionClassLibrary">
		<rdfs:subClassOf rdf:resource="&java;JavaClassLibrary"/>
		<rdfs:comment xml:lang="en">JavaLibrary implementing the javax.transaction package for J2SE 1.3</rdfs:comment>
		<rdfs:comment xml:lang="OWLManchester">platform:implementsInterface some JavaxTransactionAPI</rdfs:comment>
	</owl:Class>
	<owl:Class rdf:about="#OrgOmgCORBA_2_3ClassLibrary">
		<rdfs:subClassOf rdf:resource="&java;JavaClassLibrary"/>
		<rdfs:comment xml:lang="en">JavaLibrary implementing the org.omg.CORBA_2_3 package for J2SE 1.3</rdfs:comment>
		<rdfs:comment xml:lang="OWLManchester">platform:implementsInterface some OrgOmgCORBA_2_3API</rdfs:comment>
	</owl:Class>
	<owl:Class rdf:about="#OrgOmgCORBA_2_3PortableClassLibrary">
		<rdfs:subClassOf rdf:resource="&java;JavaClassLibrary"/>
		<rdfs:comment xml:lang="en">JavaLibrary implementing the org.omg.CORBA_2_3.portable package for J2SE 1.3</rdfs:comment>
		<rdfs:comment xml:lang="OWLManchester">platform:implementsInterface some OrgOmgCORBA_2_3PortableAPI</rdfs:comment>
	</owl:Class>
	<owl:Class rdf:about="#OrgOmgCORBAClassLibrary">
		<rdfs:subClassOf rdf:resource="&j2se-1_2;OrgOmgCORBAClassLibrary"/>
		<rdfs:comment xml:lang="en">JavaLibrary implementing the org.omg.CORBA package for J2SE 1.3</rdfs:comment>
		<rdfs:comment xml:lang="OWLManchester">platform:implementsInterface some OrgOmgCORBAAPI</rdfs:comment>
	</owl:Class>
	<owl:Class rdf:about="#OrgOmgCORBAPortableClassLibrary">
		<rdfs:subClassOf rdf:resource="&j2se-1_2;OrgOmgCORBAPortableClassLibrary"/>
		<rdfs:comment xml:lang="en">JavaLibrary implementing the org.omg.CORBA.portable package for J2SE 1.3</rdfs:comment>
		<rdfs:comment xml:lang="OWLManchester">platform:implementsInterface some OrgOmgCORBAPortableAPI</rdfs:comment>
	</owl:Class>
	<owl:Class rdf:about="#OrgOmgCORBATypeCodePackageClassLibrary">
		<owl:equivalentClass rdf:resource="&j2se-1_2;OrgOmgCORBATypeCodePackageClassLibrary"/>
		<rdfs:subClassOf rdf:resource="&java;JavaClassLibrary"/>
		<rdfs:comment xml:lang="en">JavaLibrary implementing the org.omg.CORBA.TypeCodePackage package for J2SE 1.3</rdfs:comment>
		<rdfs:comment xml:lang="OWLManchester">platform:implementsInterface some OrgOmgCORBATypeCodePackageAPI</rdfs:comment>
	</owl:Class>
	<owl:Class rdf:about="#OrgOmgCORBAORBPackageClassLibrary">
		<owl:equivalentClass rdf:resource="&j2se-1_2;OrgOmgCORBAORBPackageClassLibrary"/>
		<rdfs:subClassOf rdf:resource="&java;JavaClassLibrary"/>
		<rdfs:comment xml:lang="en">JavaLibrary implementing the org.omg.CORBA.ORBPackage package for J2SE 1.3</rdfs:comment>
		<rdfs:comment xml:lang="OWLManchester">platform:implementsInterface some OrgOmgCORBAORBPackageAPI</rdfs:comment>
	</owl:Class>
	<owl:Class rdf:about="#OrgOmgCORBADynAnyPackageClassLibrary">
		<owl:equivalentClass rdf:resource="&j2se-1_2;OrgOmgCORBADynAnyPackageClassLibrary"/>
		<rdfs:subClassOf rdf:resource="&java;JavaClassLibrary"/>
		<rdfs:comment xml:lang="en">JavaLibrary implementing the org.omg.CORBA.DynAnyPackage package for J2SE 1.3</rdfs:comment>
		<rdfs:comment xml:lang="OWLManchester">platform:implementsInterface some OrgOmgCORBADynAnyPackageAPI</rdfs:comment>
	</owl:Class>
	<owl:Class rdf:about="#OrgOmgSendingContextClassLibrary">
		<rdfs:subClassOf rdf:resource="&java;JavaClassLibrary"/>
		<rdfs:comment xml:lang="en">JavaLibrary implementing the org.omg.SendingContext package for J2SE 1.3</rdfs:comment>
		<rdfs:comment xml:lang="OWLManchester">platform:implementsInterface some OrgOmgSendingContextAPI</rdfs:comment>
	</owl:Class>
	<owl:Class rdf:about="#OrgOmgCosNamingClassLibrary">
		<rdfs:subClassOf rdf:resource="&j2se-1_2;OrgOmgCosNamingClassLibrary"/>
		<rdfs:comment xml:lang="en">JavaLibrary implementing the org.omg.CosNaming package for J2SE 1.3</rdfs:comment>
		<rdfs:comment xml:lang="OWLManchester">platform:implementsInterface some OrgOmgCosNamingAPI</rdfs:comment>
	</owl:Class>
	<owl:Class rdf:about="#OrgOmgCosNamingNamingContextPackageClassLibrary">
		<owl:equivalentClass rdf:resource="&j2se-1_2;OrgOmgCosNamingNamingContextPackageClassLibrary"/>
		<rdfs:subClassOf rdf:resource="&java;JavaClassLibrary"/>
		<rdfs:comment xml:lang="en">JavaLibrary implementing the org.omg.CosNaming.NamingContextPackage package for J2SE 1.3</rdfs:comment>
		<rdfs:comment xml:lang="OWLManchester">platform:implementsInterface some OrgOmgCosNamingNamingContextPackageAPI</rdfs:comment>
	</owl:Class>
	<owl:Class rdf:about="#OrgOmgStubJavaRmiClassLibrary">
		<rdfs:subClassOf rdf:resource="&java;JavaClassLibrary"/>
		<rdfs:comment xml:lang="en">JavaLibrary implementing the org.omg.stub.java.rmi package for J2SE 1.3</rdfs:comment>
		<rdfs:comment xml:lang="OWLManchester">platform:implementsInterface some OrgOmgStubJavaRmiAPI</rdfs:comment>
	</owl:Class>
</rdf:RDF>
