<?xml version="1.0" encoding="ISO-8859-1"?>
<!DOCTYPE rdf:RDF [
	<!ENTITY isa "http://soft.vub.ac.be/platformkit/2010/1/isa.owl#">
	<!ENTITY platform "http://soft.vub.ac.be/platformkit/2010/1/platform.owl#">
	<!ENTITY personaljava-1_1 "http://soft.vub.ac.be/platformkit/2010/1/personaljava-1_1.owl#">
	<!ENTITY java "http://soft.vub.ac.be/platformkit/2010/1/java.owl#">
	<!ENTITY xsd "http://www.w3.org/2001/XMLSchema#">
	<!ENTITY owl "http://www.w3.org/2002/07/owl#">
	<!ENTITY rdf "http://www.w3.org/1999/02/22-rdf-syntax-ns#">
	<!ENTITY rdfs "http://www.w3.org/2000/01/rdf-schema#">
]>
<rdf:RDF
	 xmlns="http://soft.vub.ac.be/platformkit/2010/1/jdk-1_1.owl#"
	 xml:base="http://soft.vub.ac.be/platformkit/2010/1/jdk-1_1.owl"
	 xmlns:isa="&isa;"
	 xmlns:platform="&platform;"
	 xmlns:personaljava-1_1="&personaljava-1_1;"
	 xmlns:java="&java;"
	 xmlns:xsd="&xsd;"
	 xmlns:owl="&owl;"
	 xmlns:rdf="&rdf;"
	 xmlns:rdfs="&rdfs;"
>

	<owl:Ontology rdf:about="">
		<owl:versionInfo>$Id$</owl:versionInfo>
		<owl:imports rdf:resource="http://soft.vub.ac.be/platformkit/2010/1/platform.owl"/>
		<owl:imports rdf:resource="http://soft.vub.ac.be/platformkit/2010/1/java.owl"/>
		<owl:imports rdf:resource="http://soft.vub.ac.be/platformkit/2010/1/personaljava-1_1.owl"/>
		<owl:imports rdf:resource="http://soft.vub.ac.be/platformkit/2010/1/isa.owl"/>
		<rdfs:comment xml:lang="en">Generated by [UML2ToSimplifiedPackageAPIOntology.atl 8080 2010-03-18 10:46:40Z dwagelaa], [UML2ToPackageAPIOntology.atl 8082 2010-03-18 21:11:00Z dwagelaa], [UML2ToAPIOntology.atl 8082 2010-03-18 21:11:00Z dwagelaa], and [UML2Comparison.atl 8082 2010-03-18 21:11:00Z dwagelaa]</rdfs:comment>
		<rdfs:comment>Dennis Wagelaar &lt;dennis.wagelaar@vub.ac.be&gt;</rdfs:comment>
		<rdfs:comment xml:lang="en">&#169; 2010, Vrije Universiteit Brussel. All rights reserved.</rdfs:comment>
		<rdfs:label xml:lang="en">JDK 1.1</rdfs:label>
	</owl:Ontology>
	<owl:Class rdf:about="#JDK1_1API">
		<rdfs:subClassOf rdf:resource="#JavaLangAPI"/>
		<rdfs:subClassOf rdf:resource="#JavaLangReflectAPI"/>
		<rdfs:subClassOf rdf:resource="#JavaIoAPI"/>
		<rdfs:subClassOf rdf:resource="#JavaNetAPI"/>
		<rdfs:subClassOf rdf:resource="#JavaUtilAPI"/>
		<rdfs:subClassOf rdf:resource="#JavaUtilZipAPI"/>
		<rdfs:subClassOf rdf:resource="#JavaTextAPI"/>
		<rdfs:subClassOf rdf:resource="#JavaTextResourcesAPI"/>
		<rdfs:subClassOf rdf:resource="#JavaMathAPI"/>
		<rdfs:subClassOf rdf:resource="#JavaSecurityAPI"/>
		<rdfs:subClassOf rdf:resource="#JavaSecurityAclAPI"/>
		<rdfs:subClassOf rdf:resource="#JavaSecurityInterfacesAPI"/>
		<rdfs:subClassOf rdf:resource="#JavaAwtAPI"/>
		<rdfs:subClassOf rdf:resource="#JavaAwtImageAPI"/>
		<rdfs:subClassOf rdf:resource="#JavaAwtDatatransferAPI"/>
		<rdfs:subClassOf rdf:resource="#JavaAwtEventAPI"/>
		<rdfs:subClassOf rdf:resource="#JavaAppletAPI"/>
		<rdfs:subClassOf rdf:resource="#JavaSqlAPI"/>
		<rdfs:subClassOf rdf:resource="#JavaRmiAPI"/>
		<rdfs:subClassOf rdf:resource="#JavaRmiRegistryAPI"/>
		<rdfs:subClassOf rdf:resource="#JavaRmiDgcAPI"/>
		<rdfs:subClassOf rdf:resource="#JavaRmiServerAPI"/>
		<rdfs:subClassOf rdf:resource="#JavaBeansAPI"/>
		<rdfs:subClassOf rdf:resource="&personaljava-1_1;PersonalJava1_1API"/>
		<rdfs:comment xml:lang="en">JDK 1.1 API</rdfs:comment>
		<rdfs:comment xml:lang="OWLManchester">platform:comprisesInterfacePart some JavaLang and platform:comprisesInterfacePart some JavaLangReflect and platform:comprisesInterfacePart some JavaIo and platform:comprisesInterfacePart some JavaNet and platform:comprisesInterfacePart some JavaUtil and platform:comprisesInterfacePart some JavaUtilZip and platform:comprisesInterfacePart some JavaText and platform:comprisesInterfacePart some JavaTextResources and platform:comprisesInterfacePart some JavaMath and platform:comprisesInterfacePart some JavaSecurity and platform:comprisesInterfacePart some JavaSecurityAcl and platform:comprisesInterfacePart some JavaSecurityInterfaces and platform:comprisesInterfacePart some JavaAwt and platform:comprisesInterfacePart some JavaAwtImage and platform:comprisesInterfacePart some JavaAwtDatatransfer and platform:comprisesInterfacePart some JavaAwtEvent and platform:comprisesInterfacePart some JavaApplet and platform:comprisesInterfacePart some JavaSql and platform:comprisesInterfacePart some JavaRmi and platform:comprisesInterfacePart some JavaRmiRegistry and platform:comprisesInterfacePart some JavaRmiDgc and platform:comprisesInterfacePart some JavaRmiServer and platform:comprisesInterfacePart some JavaBeans</rdfs:comment>
	</owl:Class>
	<owl:Class rdf:about="#JDK1_1ClassLibrary">
		<rdfs:subClassOf rdf:resource="#JavaLangClassLibrary"/>
		<rdfs:subClassOf rdf:resource="#JavaLangReflectClassLibrary"/>
		<rdfs:subClassOf rdf:resource="#JavaIoClassLibrary"/>
		<rdfs:subClassOf rdf:resource="#JavaNetClassLibrary"/>
		<rdfs:subClassOf rdf:resource="#JavaUtilClassLibrary"/>
		<rdfs:subClassOf rdf:resource="#JavaUtilZipClassLibrary"/>
		<rdfs:subClassOf rdf:resource="#JavaTextClassLibrary"/>
		<rdfs:subClassOf rdf:resource="#JavaTextResourcesClassLibrary"/>
		<rdfs:subClassOf rdf:resource="#JavaMathClassLibrary"/>
		<rdfs:subClassOf rdf:resource="#JavaSecurityClassLibrary"/>
		<rdfs:subClassOf rdf:resource="#JavaSecurityAclClassLibrary"/>
		<rdfs:subClassOf rdf:resource="#JavaSecurityInterfacesClassLibrary"/>
		<rdfs:subClassOf rdf:resource="#JavaAwtClassLibrary"/>
		<rdfs:subClassOf rdf:resource="#JavaAwtImageClassLibrary"/>
		<rdfs:subClassOf rdf:resource="#JavaAwtDatatransferClassLibrary"/>
		<rdfs:subClassOf rdf:resource="#JavaAwtEventClassLibrary"/>
		<rdfs:subClassOf rdf:resource="#JavaAppletClassLibrary"/>
		<rdfs:subClassOf rdf:resource="#JavaSqlClassLibrary"/>
		<rdfs:subClassOf rdf:resource="#JavaRmiClassLibrary"/>
		<rdfs:subClassOf rdf:resource="#JavaRmiRegistryClassLibrary"/>
		<rdfs:subClassOf rdf:resource="#JavaRmiDgcClassLibrary"/>
		<rdfs:subClassOf rdf:resource="#JavaRmiServerClassLibrary"/>
		<rdfs:subClassOf rdf:resource="#JavaBeansClassLibrary"/>
		<rdfs:subClassOf rdf:resource="&personaljava-1_1;PersonalJava1_1ClassLibrary"/>
		<rdfs:comment xml:lang="en">Java class library implementing the JDK 1.1 API</rdfs:comment>
		<rdfs:comment xml:lang="OWLManchester">platform:implementsInterface some JDK1_1API</rdfs:comment>
	</owl:Class>
	<owl:Class rdf:about="#JDK1_1BytecodeFormat">
		<owl:equivalentClass rdf:resource="&personaljava-1_1;PersonalJava1_1BytecodeFormat"/>
		<rdfs:subClassOf rdf:resource="&isa;JavaBytecode"/>
		<rdfs:comment xml:lang="en">JDK 1.1 bytecode format</rdfs:comment>
		<rdfs:comment xml:lang="OWLManchester">java:majorVersionNumber some xsd:integer[>="45"^^xsd:integer] and java:preverified value false</rdfs:comment>
	</owl:Class>
	<JDK1_1BytecodeFormat rdf:about="#theJDK1_1BytecodeFormat">
		<java:preverified rdf:datatype="http://www.w3.org/2001/XMLSchema#boolean">false</java:preverified>
		<java:minorVersionNumber rdf:datatype="http://www.w3.org/2001/XMLSchema#integer">3</java:minorVersionNumber>
		<java:majorVersionNumber rdf:datatype="http://www.w3.org/2001/XMLSchema#integer">45</java:majorVersionNumber>
	</JDK1_1BytecodeFormat>
	<JDK1_1API rdf:about="#theJDK1_1API">
		<platform:comprisesInterfacePart rdf:resource="#theJavaBeansPart"/>
		<platform:comprisesInterfacePart rdf:resource="#theJavaRmiServerPart"/>
		<platform:comprisesInterfacePart rdf:resource="#theJavaRmiDgcPart"/>
		<platform:comprisesInterfacePart rdf:resource="#theJavaRmiRegistryPart"/>
		<platform:comprisesInterfacePart rdf:resource="#theJavaRmiPart"/>
		<platform:comprisesInterfacePart rdf:resource="#theJavaSqlPart"/>
		<platform:comprisesInterfacePart rdf:resource="#theJavaAppletPart"/>
		<platform:comprisesInterfacePart rdf:resource="#theJavaAwtEventPart"/>
		<platform:comprisesInterfacePart rdf:resource="#theJavaAwtDatatransferPart"/>
		<platform:comprisesInterfacePart rdf:resource="#theJavaAwtImagePart"/>
		<platform:comprisesInterfacePart rdf:resource="#theJavaAwtPart"/>
		<platform:comprisesInterfacePart rdf:resource="#theJavaSecurityInterfacesPart"/>
		<platform:comprisesInterfacePart rdf:resource="#theJavaSecurityAclPart"/>
		<platform:comprisesInterfacePart rdf:resource="#theJavaSecurityPart"/>
		<platform:comprisesInterfacePart rdf:resource="#theJavaMathPart"/>
		<platform:comprisesInterfacePart rdf:resource="#theJavaTextResourcesPart"/>
		<platform:comprisesInterfacePart rdf:resource="#theJavaTextPart"/>
		<platform:comprisesInterfacePart rdf:resource="#theJavaUtilZipPart"/>
		<platform:comprisesInterfacePart rdf:resource="#theJavaUtilPart"/>
		<platform:comprisesInterfacePart rdf:resource="#theJavaNetPart"/>
		<platform:comprisesInterfacePart rdf:resource="#theJavaIoPart"/>
		<platform:comprisesInterfacePart rdf:resource="#theJavaLangReflectPart"/>
		<platform:comprisesInterfacePart rdf:resource="#theJavaLangPart"/>
	</JDK1_1API>
	<owl:Class rdf:about="#JDK1_1VM">
		<owl:equivalentClass>
			<owl:Restriction>
				<owl:onProperty rdf:resource="&platform;implementsInterface"/>
				<owl:someValuesFrom rdf:resource="#JDK1_1BytecodeFormat"/>
			</owl:Restriction>
		</owl:equivalentClass>
		<rdfs:subClassOf rdf:resource="&java;JavaVM"/>
		<rdfs:comment xml:lang="en">JDK 1.1 virtual machine</rdfs:comment>
	</owl:Class>
	<owl:Class rdf:about="#JDK1_1JRE">
		<owl:equivalentClass>
			<owl:Class >
				<owl:intersectionOf rdf:parseType="Collection">
					<owl:Restriction>
						<owl:onProperty rdf:resource="&platform;providesFeature"/>
						<owl:someValuesFrom rdf:resource="#JDK1_1ClassLibrary"/>
					</owl:Restriction>
					<owl:Restriction>
						<owl:onProperty rdf:resource="&platform;providesFeature"/>
						<owl:someValuesFrom rdf:resource="#JDK1_1VM"/>
					</owl:Restriction>
				</owl:intersectionOf>
			</owl:Class>
		</owl:equivalentClass>
		<rdfs:subClassOf rdf:resource="&java;JRE"/>
		<rdfs:comment xml:lang="en">JDK 1.1 Java Runtime Environment</rdfs:comment>
	</owl:Class>
	<owl:Class rdf:about="#JavaLang">
		<owl:equivalentClass rdf:resource="&personaljava-1_1;JavaLang"/>
		<rdfs:subClassOf rdf:resource="&java;JavaAPIPart"/>
		<rdfs:seeAlso rdf:resource="#JavaUtil"/>
		<rdfs:seeAlso rdf:resource="#JavaLangReflect"/>
		<rdfs:seeAlso rdf:resource="#JavaNet"/>
		<rdfs:seeAlso rdf:resource="#JavaIo"/>
		<rdfs:comment xml:lang="en">Java API part implementing the java.lang package for JDK 1.1</rdfs:comment>
	</owl:Class>
	<owl:Class rdf:about="#JavaLangReflect">
		<owl:equivalentClass rdf:resource="&personaljava-1_1;JavaLangReflect"/>
		<rdfs:subClassOf rdf:resource="&java;JavaAPIPart"/>
		<rdfs:seeAlso rdf:resource="#JavaLang"/>
		<rdfs:comment xml:lang="en">Java API part implementing the java.lang.reflect package for JDK 1.1</rdfs:comment>
	</owl:Class>
	<owl:Class rdf:about="#JavaIo">
		<rdfs:subClassOf rdf:resource="&personaljava-1_1;JavaIo"/>
		<rdfs:seeAlso rdf:resource="#JavaLang"/>
		<rdfs:seeAlso rdf:resource="#JavaUtil"/>
		<rdfs:comment xml:lang="en">Java API part implementing the java.io package for JDK 1.1</rdfs:comment>
	</owl:Class>
	<owl:Class rdf:about="#JavaNet">
		<owl:equivalentClass rdf:resource="&personaljava-1_1;JavaNet"/>
		<rdfs:subClassOf rdf:resource="&java;JavaAPIPart"/>
		<rdfs:seeAlso rdf:resource="#JavaLang"/>
		<rdfs:seeAlso rdf:resource="#JavaIo"/>
		<rdfs:comment xml:lang="en">Java API part implementing the java.net package for JDK 1.1</rdfs:comment>
	</owl:Class>
	<owl:Class rdf:about="#JavaUtil">
		<owl:equivalentClass rdf:resource="&personaljava-1_1;JavaUtil"/>
		<rdfs:subClassOf rdf:resource="&java;JavaAPIPart"/>
		<rdfs:seeAlso rdf:resource="#JavaLang"/>
		<rdfs:seeAlso rdf:resource="#JavaIo"/>
		<rdfs:comment xml:lang="en">Java API part implementing the java.util package for JDK 1.1</rdfs:comment>
	</owl:Class>
	<owl:Class rdf:about="#JavaUtilZip">
		<rdfs:subClassOf rdf:resource="&personaljava-1_1;JavaUtilZip"/>
		<rdfs:seeAlso rdf:resource="#JavaLang"/>
		<rdfs:seeAlso rdf:resource="#JavaUtil"/>
		<rdfs:seeAlso rdf:resource="#JavaIo"/>
		<rdfs:comment xml:lang="en">Java API part implementing the java.util.zip package for JDK 1.1</rdfs:comment>
	</owl:Class>
	<owl:Class rdf:about="#JavaText">
		<owl:equivalentClass rdf:resource="&personaljava-1_1;JavaText"/>
		<rdfs:subClassOf rdf:resource="&java;JavaAPIPart"/>
		<rdfs:seeAlso rdf:resource="#JavaLang"/>
		<rdfs:seeAlso rdf:resource="#JavaUtil"/>
		<rdfs:seeAlso rdf:resource="#JavaIo"/>
		<rdfs:comment xml:lang="en">Java API part implementing the java.text package for JDK 1.1</rdfs:comment>
	</owl:Class>
	<owl:Class rdf:about="#JavaTextResources">
		<rdfs:subClassOf rdf:resource="&personaljava-1_1;JavaTextResources"/>
		<rdfs:seeAlso rdf:resource="#JavaLang"/>
		<rdfs:seeAlso rdf:resource="#JavaUtil"/>
		<rdfs:comment xml:lang="en">Java API part implementing the java.text.resources package for JDK 1.1</rdfs:comment>
	</owl:Class>
	<owl:Class rdf:about="#JavaMath">
		<rdfs:subClassOf rdf:resource="&java;JavaAPIPart"/>
		<rdfs:seeAlso rdf:resource="#JavaLang"/>
		<rdfs:seeAlso rdf:resource="#JavaUtil"/>
		<rdfs:comment xml:lang="en">Java API part implementing the java.math package for JDK 1.1</rdfs:comment>
	</owl:Class>
	<owl:Class rdf:about="#JavaSecurity">
		<rdfs:subClassOf rdf:resource="&java;JavaAPIPart"/>
		<rdfs:seeAlso rdf:resource="#JavaUtil"/>
		<rdfs:seeAlso rdf:resource="#JavaLang"/>
		<rdfs:seeAlso rdf:resource="#JavaIo"/>
		<rdfs:comment xml:lang="en">Java API part implementing the java.security package for JDK 1.1</rdfs:comment>
	</owl:Class>
	<owl:Class rdf:about="#JavaSecurityAcl">
		<rdfs:subClassOf rdf:resource="&java;JavaAPIPart"/>
		<rdfs:seeAlso rdf:resource="#JavaLang"/>
		<rdfs:seeAlso rdf:resource="#JavaSecurity"/>
		<rdfs:seeAlso rdf:resource="#JavaUtil"/>
		<rdfs:comment xml:lang="en">Java API part implementing the java.security.acl package for JDK 1.1</rdfs:comment>
	</owl:Class>
	<owl:Class rdf:about="#JavaSecurityInterfaces">
		<rdfs:subClassOf rdf:resource="&java;JavaAPIPart"/>
		<rdfs:seeAlso rdf:resource="#JavaSecurity"/>
		<rdfs:seeAlso rdf:resource="#JavaMath"/>
		<rdfs:comment xml:lang="en">Java API part implementing the java.security.interfaces package for JDK 1.1</rdfs:comment>
	</owl:Class>
	<owl:Class rdf:about="#JavaAwt">
		<rdfs:subClassOf rdf:resource="&personaljava-1_1;JavaAwt"/>
		<rdfs:seeAlso rdf:resource="#JavaAwtEvent"/>
		<rdfs:seeAlso rdf:resource="#JavaIo"/>
		<rdfs:seeAlso rdf:resource="#JavaAwtImage"/>
		<rdfs:seeAlso rdf:resource="#JavaUtil"/>
		<rdfs:seeAlso rdf:resource="#JavaLang"/>
		<rdfs:seeAlso rdf:resource="#JavaNet"/>
		<rdfs:seeAlso rdf:resource="#JavaAwtDatatransfer"/>
		<rdfs:comment xml:lang="en">Java API part implementing the java.awt package for JDK 1.1</rdfs:comment>
	</owl:Class>
	<owl:Class rdf:about="#JavaAwtImage">
		<owl:equivalentClass rdf:resource="&personaljava-1_1;JavaAwtImage"/>
		<rdfs:subClassOf rdf:resource="&java;JavaAPIPart"/>
		<rdfs:seeAlso rdf:resource="#JavaLang"/>
		<rdfs:seeAlso rdf:resource="#JavaUtil"/>
		<rdfs:seeAlso rdf:resource="#JavaAwt"/>
		<rdfs:comment xml:lang="en">Java API part implementing the java.awt.image package for JDK 1.1</rdfs:comment>
	</owl:Class>
	<owl:Class rdf:about="#JavaAwtDatatransfer">
		<owl:equivalentClass rdf:resource="&personaljava-1_1;JavaAwtDatatransfer"/>
		<rdfs:subClassOf rdf:resource="&java;JavaAPIPart"/>
		<rdfs:seeAlso rdf:resource="#JavaLang"/>
		<rdfs:comment xml:lang="en">Java API part implementing the java.awt.datatransfer package for JDK 1.1</rdfs:comment>
	</owl:Class>
	<owl:Class rdf:about="#JavaAwtEvent">
		<owl:equivalentClass rdf:resource="&personaljava-1_1;JavaAwtEvent"/>
		<rdfs:subClassOf rdf:resource="&java;JavaAPIPart"/>
		<rdfs:seeAlso rdf:resource="#JavaLang"/>
		<rdfs:seeAlso rdf:resource="#JavaUtil"/>
		<rdfs:seeAlso rdf:resource="#JavaAwt"/>
		<rdfs:comment xml:lang="en">Java API part implementing the java.awt.event package for JDK 1.1</rdfs:comment>
	</owl:Class>
	<owl:Class rdf:about="#JavaApplet">
		<owl:equivalentClass rdf:resource="&personaljava-1_1;JavaApplet"/>
		<rdfs:subClassOf rdf:resource="&java;JavaAPIPart"/>
		<rdfs:seeAlso rdf:resource="#JavaLang"/>
		<rdfs:seeAlso rdf:resource="#JavaUtil"/>
		<rdfs:seeAlso rdf:resource="#JavaNet"/>
		<rdfs:seeAlso rdf:resource="#JavaAwt"/>
		<rdfs:comment xml:lang="en">Java API part implementing the java.applet package for JDK 1.1</rdfs:comment>
	</owl:Class>
	<owl:Class rdf:about="#JavaSql">
		<rdfs:subClassOf rdf:resource="&java;JavaAPIPart"/>
		<rdfs:seeAlso rdf:resource="#JavaLang"/>
		<rdfs:seeAlso rdf:resource="#JavaUtil"/>
		<rdfs:seeAlso rdf:resource="#JavaMath"/>
		<rdfs:seeAlso rdf:resource="#JavaIo"/>
		<rdfs:comment xml:lang="en">Java API part implementing the java.sql package for JDK 1.1</rdfs:comment>
	</owl:Class>
	<owl:Class rdf:about="#JavaRmi">
		<rdfs:subClassOf rdf:resource="&java;JavaAPIPart"/>
		<rdfs:seeAlso rdf:resource="#JavaLang"/>
		<rdfs:seeAlso rdf:resource="#JavaNet"/>
		<rdfs:seeAlso rdf:resource="#JavaIo"/>
		<rdfs:comment xml:lang="en">Java API part implementing the java.rmi package for JDK 1.1</rdfs:comment>
	</owl:Class>
	<owl:Class rdf:about="#JavaRmiRegistry">
		<rdfs:subClassOf rdf:resource="&java;JavaAPIPart"/>
		<rdfs:seeAlso rdf:resource="#JavaLang"/>
		<rdfs:seeAlso rdf:resource="#JavaRmi"/>
		<rdfs:comment xml:lang="en">Java API part implementing the java.rmi.registry package for JDK 1.1</rdfs:comment>
	</owl:Class>
	<owl:Class rdf:about="#JavaRmiDgc">
		<rdfs:subClassOf rdf:resource="&java;JavaAPIPart"/>
		<rdfs:seeAlso rdf:resource="#JavaLang"/>
		<rdfs:seeAlso rdf:resource="#JavaRmi"/>
		<rdfs:seeAlso rdf:resource="#JavaIo"/>
		<rdfs:comment xml:lang="en">Java API part implementing the java.rmi.dgc package for JDK 1.1</rdfs:comment>
	</owl:Class>
	<owl:Class rdf:about="#JavaRmiServer">
		<rdfs:subClassOf rdf:resource="&java;JavaAPIPart"/>
		<rdfs:seeAlso rdf:resource="#JavaLang"/>
		<rdfs:seeAlso rdf:resource="#JavaNet"/>
		<rdfs:seeAlso rdf:resource="#JavaRmi"/>
		<rdfs:seeAlso rdf:resource="#JavaIo"/>
		<rdfs:comment xml:lang="en">Java API part implementing the java.rmi.server package for JDK 1.1</rdfs:comment>
	</owl:Class>
	<owl:Class rdf:about="#JavaBeans">
		<owl:equivalentClass rdf:resource="&personaljava-1_1;JavaBeans"/>
		<rdfs:subClassOf rdf:resource="&java;JavaAPIPart"/>
		<rdfs:seeAlso rdf:resource="#JavaUtil"/>
		<rdfs:seeAlso rdf:resource="#JavaLangReflect"/>
		<rdfs:seeAlso rdf:resource="#JavaLang"/>
		<rdfs:seeAlso rdf:resource="#JavaIo"/>
		<rdfs:seeAlso rdf:resource="#JavaAwt"/>
		<rdfs:comment xml:lang="en">Java API part implementing the java.beans package for JDK 1.1</rdfs:comment>
	</owl:Class>
	<owl:Class rdf:about="#JavaLangAPI">
		<owl:equivalentClass rdf:resource="&personaljava-1_1;JavaLangAPI"/>
		<rdfs:subClassOf rdf:resource="&java;JavaAPI"/>
		<rdfs:comment xml:lang="en">JavaLibrary implementing the java.lang package for JDK 1.1</rdfs:comment>
		<rdfs:comment xml:lang="OWLManchester">platform:comprisesInterfacePart some JavaLang</rdfs:comment>
	</owl:Class>
	<owl:Class rdf:about="#JavaLangReflectAPI">
		<owl:equivalentClass rdf:resource="&personaljava-1_1;JavaLangReflectAPI"/>
		<rdfs:subClassOf rdf:resource="&java;JavaAPI"/>
		<rdfs:comment xml:lang="en">JavaLibrary implementing the java.lang.reflect package for JDK 1.1</rdfs:comment>
		<rdfs:comment xml:lang="OWLManchester">platform:comprisesInterfacePart some JavaLangReflect</rdfs:comment>
	</owl:Class>
	<owl:Class rdf:about="#JavaIoAPI">
		<rdfs:subClassOf rdf:resource="&personaljava-1_1;JavaIoAPI"/>
		<rdfs:comment xml:lang="en">JavaLibrary implementing the java.io package for JDK 1.1</rdfs:comment>
		<rdfs:comment xml:lang="OWLManchester">platform:comprisesInterfacePart some JavaIo</rdfs:comment>
	</owl:Class>
	<owl:Class rdf:about="#JavaNetAPI">
		<owl:equivalentClass rdf:resource="&personaljava-1_1;JavaNetAPI"/>
		<rdfs:subClassOf rdf:resource="&java;JavaAPI"/>
		<rdfs:comment xml:lang="en">JavaLibrary implementing the java.net package for JDK 1.1</rdfs:comment>
		<rdfs:comment xml:lang="OWLManchester">platform:comprisesInterfacePart some JavaNet</rdfs:comment>
	</owl:Class>
	<owl:Class rdf:about="#JavaUtilAPI">
		<owl:equivalentClass rdf:resource="&personaljava-1_1;JavaUtilAPI"/>
		<rdfs:subClassOf rdf:resource="&java;JavaAPI"/>
		<rdfs:comment xml:lang="en">JavaLibrary implementing the java.util package for JDK 1.1</rdfs:comment>
		<rdfs:comment xml:lang="OWLManchester">platform:comprisesInterfacePart some JavaUtil</rdfs:comment>
	</owl:Class>
	<owl:Class rdf:about="#JavaUtilZipAPI">
		<rdfs:subClassOf rdf:resource="&personaljava-1_1;JavaUtilZipAPI"/>
		<rdfs:comment xml:lang="en">JavaLibrary implementing the java.util.zip package for JDK 1.1</rdfs:comment>
		<rdfs:comment xml:lang="OWLManchester">platform:comprisesInterfacePart some JavaUtilZip</rdfs:comment>
	</owl:Class>
	<owl:Class rdf:about="#JavaTextAPI">
		<owl:equivalentClass rdf:resource="&personaljava-1_1;JavaTextAPI"/>
		<rdfs:subClassOf rdf:resource="&java;JavaAPI"/>
		<rdfs:comment xml:lang="en">JavaLibrary implementing the java.text package for JDK 1.1</rdfs:comment>
		<rdfs:comment xml:lang="OWLManchester">platform:comprisesInterfacePart some JavaText</rdfs:comment>
	</owl:Class>
	<owl:Class rdf:about="#JavaTextResourcesAPI">
		<rdfs:subClassOf rdf:resource="&personaljava-1_1;JavaTextResourcesAPI"/>
		<rdfs:comment xml:lang="en">JavaLibrary implementing the java.text.resources package for JDK 1.1</rdfs:comment>
		<rdfs:comment xml:lang="OWLManchester">platform:comprisesInterfacePart some JavaTextResources</rdfs:comment>
	</owl:Class>
	<owl:Class rdf:about="#JavaMathAPI">
		<rdfs:subClassOf rdf:resource="&java;JavaAPI"/>
		<rdfs:comment xml:lang="en">JavaLibrary implementing the java.math package for JDK 1.1</rdfs:comment>
		<rdfs:comment xml:lang="OWLManchester">platform:comprisesInterfacePart some JavaMath</rdfs:comment>
	</owl:Class>
	<owl:Class rdf:about="#JavaSecurityAPI">
		<rdfs:subClassOf rdf:resource="&java;JavaAPI"/>
		<rdfs:comment xml:lang="en">JavaLibrary implementing the java.security package for JDK 1.1</rdfs:comment>
		<rdfs:comment xml:lang="OWLManchester">platform:comprisesInterfacePart some JavaSecurity</rdfs:comment>
	</owl:Class>
	<owl:Class rdf:about="#JavaSecurityAclAPI">
		<rdfs:subClassOf rdf:resource="&java;JavaAPI"/>
		<rdfs:comment xml:lang="en">JavaLibrary implementing the java.security.acl package for JDK 1.1</rdfs:comment>
		<rdfs:comment xml:lang="OWLManchester">platform:comprisesInterfacePart some JavaSecurityAcl</rdfs:comment>
	</owl:Class>
	<owl:Class rdf:about="#JavaSecurityInterfacesAPI">
		<rdfs:subClassOf rdf:resource="&java;JavaAPI"/>
		<rdfs:comment xml:lang="en">JavaLibrary implementing the java.security.interfaces package for JDK 1.1</rdfs:comment>
		<rdfs:comment xml:lang="OWLManchester">platform:comprisesInterfacePart some JavaSecurityInterfaces</rdfs:comment>
	</owl:Class>
	<owl:Class rdf:about="#JavaAwtAPI">
		<rdfs:subClassOf rdf:resource="&personaljava-1_1;JavaAwtAPI"/>
		<rdfs:comment xml:lang="en">JavaLibrary implementing the java.awt package for JDK 1.1</rdfs:comment>
		<rdfs:comment xml:lang="OWLManchester">platform:comprisesInterfacePart some JavaAwt</rdfs:comment>
	</owl:Class>
	<owl:Class rdf:about="#JavaAwtImageAPI">
		<owl:equivalentClass rdf:resource="&personaljava-1_1;JavaAwtImageAPI"/>
		<rdfs:subClassOf rdf:resource="&java;JavaAPI"/>
		<rdfs:comment xml:lang="en">JavaLibrary implementing the java.awt.image package for JDK 1.1</rdfs:comment>
		<rdfs:comment xml:lang="OWLManchester">platform:comprisesInterfacePart some JavaAwtImage</rdfs:comment>
	</owl:Class>
	<owl:Class rdf:about="#JavaAwtDatatransferAPI">
		<owl:equivalentClass rdf:resource="&personaljava-1_1;JavaAwtDatatransferAPI"/>
		<rdfs:subClassOf rdf:resource="&java;JavaAPI"/>
		<rdfs:comment xml:lang="en">JavaLibrary implementing the java.awt.datatransfer package for JDK 1.1</rdfs:comment>
		<rdfs:comment xml:lang="OWLManchester">platform:comprisesInterfacePart some JavaAwtDatatransfer</rdfs:comment>
	</owl:Class>
	<owl:Class rdf:about="#JavaAwtEventAPI">
		<owl:equivalentClass rdf:resource="&personaljava-1_1;JavaAwtEventAPI"/>
		<rdfs:subClassOf rdf:resource="&java;JavaAPI"/>
		<rdfs:comment xml:lang="en">JavaLibrary implementing the java.awt.event package for JDK 1.1</rdfs:comment>
		<rdfs:comment xml:lang="OWLManchester">platform:comprisesInterfacePart some JavaAwtEvent</rdfs:comment>
	</owl:Class>
	<owl:Class rdf:about="#JavaAppletAPI">
		<owl:equivalentClass rdf:resource="&personaljava-1_1;JavaAppletAPI"/>
		<rdfs:subClassOf rdf:resource="&java;JavaAPI"/>
		<rdfs:comment xml:lang="en">JavaLibrary implementing the java.applet package for JDK 1.1</rdfs:comment>
		<rdfs:comment xml:lang="OWLManchester">platform:comprisesInterfacePart some JavaApplet</rdfs:comment>
	</owl:Class>
	<owl:Class rdf:about="#JavaSqlAPI">
		<rdfs:subClassOf rdf:resource="&java;JavaAPI"/>
		<rdfs:comment xml:lang="en">JavaLibrary implementing the java.sql package for JDK 1.1</rdfs:comment>
		<rdfs:comment xml:lang="OWLManchester">platform:comprisesInterfacePart some JavaSql</rdfs:comment>
	</owl:Class>
	<owl:Class rdf:about="#JavaRmiAPI">
		<rdfs:subClassOf rdf:resource="&java;JavaAPI"/>
		<rdfs:comment xml:lang="en">JavaLibrary implementing the java.rmi package for JDK 1.1</rdfs:comment>
		<rdfs:comment xml:lang="OWLManchester">platform:comprisesInterfacePart some JavaRmi</rdfs:comment>
	</owl:Class>
	<owl:Class rdf:about="#JavaRmiRegistryAPI">
		<rdfs:subClassOf rdf:resource="&java;JavaAPI"/>
		<rdfs:comment xml:lang="en">JavaLibrary implementing the java.rmi.registry package for JDK 1.1</rdfs:comment>
		<rdfs:comment xml:lang="OWLManchester">platform:comprisesInterfacePart some JavaRmiRegistry</rdfs:comment>
	</owl:Class>
	<owl:Class rdf:about="#JavaRmiDgcAPI">
		<rdfs:subClassOf rdf:resource="&java;JavaAPI"/>
		<rdfs:comment xml:lang="en">JavaLibrary implementing the java.rmi.dgc package for JDK 1.1</rdfs:comment>
		<rdfs:comment xml:lang="OWLManchester">platform:comprisesInterfacePart some JavaRmiDgc</rdfs:comment>
	</owl:Class>
	<owl:Class rdf:about="#JavaRmiServerAPI">
		<rdfs:subClassOf rdf:resource="&java;JavaAPI"/>
		<rdfs:comment xml:lang="en">JavaLibrary implementing the java.rmi.server package for JDK 1.1</rdfs:comment>
		<rdfs:comment xml:lang="OWLManchester">platform:comprisesInterfacePart some JavaRmiServer</rdfs:comment>
	</owl:Class>
	<owl:Class rdf:about="#JavaBeansAPI">
		<owl:equivalentClass rdf:resource="&personaljava-1_1;JavaBeansAPI"/>
		<rdfs:subClassOf rdf:resource="&java;JavaAPI"/>
		<rdfs:comment xml:lang="en">JavaLibrary implementing the java.beans package for JDK 1.1</rdfs:comment>
		<rdfs:comment xml:lang="OWLManchester">platform:comprisesInterfacePart some JavaBeans</rdfs:comment>
	</owl:Class>
	<JavaLang rdf:about="#theJavaLangPart">
	</JavaLang>
	<JavaLangReflect rdf:about="#theJavaLangReflectPart">
	</JavaLangReflect>
	<JavaIo rdf:about="#theJavaIoPart">
	</JavaIo>
	<JavaNet rdf:about="#theJavaNetPart">
	</JavaNet>
	<JavaUtil rdf:about="#theJavaUtilPart">
	</JavaUtil>
	<JavaUtilZip rdf:about="#theJavaUtilZipPart">
	</JavaUtilZip>
	<JavaText rdf:about="#theJavaTextPart">
	</JavaText>
	<JavaTextResources rdf:about="#theJavaTextResourcesPart">
	</JavaTextResources>
	<JavaMath rdf:about="#theJavaMathPart">
	</JavaMath>
	<JavaSecurity rdf:about="#theJavaSecurityPart">
	</JavaSecurity>
	<JavaSecurityAcl rdf:about="#theJavaSecurityAclPart">
	</JavaSecurityAcl>
	<JavaSecurityInterfaces rdf:about="#theJavaSecurityInterfacesPart">
	</JavaSecurityInterfaces>
	<JavaAwt rdf:about="#theJavaAwtPart">
	</JavaAwt>
	<JavaAwtImage rdf:about="#theJavaAwtImagePart">
	</JavaAwtImage>
	<JavaAwtDatatransfer rdf:about="#theJavaAwtDatatransferPart">
	</JavaAwtDatatransfer>
	<JavaAwtEvent rdf:about="#theJavaAwtEventPart">
	</JavaAwtEvent>
	<JavaApplet rdf:about="#theJavaAppletPart">
	</JavaApplet>
	<JavaSql rdf:about="#theJavaSqlPart">
	</JavaSql>
	<JavaRmi rdf:about="#theJavaRmiPart">
	</JavaRmi>
	<JavaRmiRegistry rdf:about="#theJavaRmiRegistryPart">
	</JavaRmiRegistry>
	<JavaRmiDgc rdf:about="#theJavaRmiDgcPart">
	</JavaRmiDgc>
	<JavaRmiServer rdf:about="#theJavaRmiServerPart">
	</JavaRmiServer>
	<JavaBeans rdf:about="#theJavaBeansPart">
	</JavaBeans>
	<owl:Class rdf:about="#JavaLangClassLibrary">
		<owl:equivalentClass rdf:resource="&personaljava-1_1;JavaLangClassLibrary"/>
		<rdfs:subClassOf rdf:resource="&java;JavaClassLibrary"/>
		<rdfs:comment xml:lang="en">JavaLibrary implementing the java.lang package for JDK 1.1</rdfs:comment>
		<rdfs:comment xml:lang="OWLManchester">platform:implementsInterface some JavaLangAPI</rdfs:comment>
	</owl:Class>
	<owl:Class rdf:about="#JavaLangReflectClassLibrary">
		<owl:equivalentClass rdf:resource="&personaljava-1_1;JavaLangReflectClassLibrary"/>
		<rdfs:subClassOf rdf:resource="&java;JavaClassLibrary"/>
		<rdfs:comment xml:lang="en">JavaLibrary implementing the java.lang.reflect package for JDK 1.1</rdfs:comment>
		<rdfs:comment xml:lang="OWLManchester">platform:implementsInterface some JavaLangReflectAPI</rdfs:comment>
	</owl:Class>
	<owl:Class rdf:about="#JavaIoClassLibrary">
		<rdfs:subClassOf rdf:resource="&personaljava-1_1;JavaIoClassLibrary"/>
		<rdfs:comment xml:lang="en">JavaLibrary implementing the java.io package for JDK 1.1</rdfs:comment>
		<rdfs:comment xml:lang="OWLManchester">platform:implementsInterface some JavaIoAPI</rdfs:comment>
	</owl:Class>
	<owl:Class rdf:about="#JavaNetClassLibrary">
		<owl:equivalentClass rdf:resource="&personaljava-1_1;JavaNetClassLibrary"/>
		<rdfs:subClassOf rdf:resource="&java;JavaClassLibrary"/>
		<rdfs:comment xml:lang="en">JavaLibrary implementing the java.net package for JDK 1.1</rdfs:comment>
		<rdfs:comment xml:lang="OWLManchester">platform:implementsInterface some JavaNetAPI</rdfs:comment>
	</owl:Class>
	<owl:Class rdf:about="#JavaUtilClassLibrary">
		<owl:equivalentClass rdf:resource="&personaljava-1_1;JavaUtilClassLibrary"/>
		<rdfs:subClassOf rdf:resource="&java;JavaClassLibrary"/>
		<rdfs:comment xml:lang="en">JavaLibrary implementing the java.util package for JDK 1.1</rdfs:comment>
		<rdfs:comment xml:lang="OWLManchester">platform:implementsInterface some JavaUtilAPI</rdfs:comment>
	</owl:Class>
	<owl:Class rdf:about="#JavaUtilZipClassLibrary">
		<rdfs:subClassOf rdf:resource="&personaljava-1_1;JavaUtilZipClassLibrary"/>
		<rdfs:comment xml:lang="en">JavaLibrary implementing the java.util.zip package for JDK 1.1</rdfs:comment>
		<rdfs:comment xml:lang="OWLManchester">platform:implementsInterface some JavaUtilZipAPI</rdfs:comment>
	</owl:Class>
	<owl:Class rdf:about="#JavaTextClassLibrary">
		<owl:equivalentClass rdf:resource="&personaljava-1_1;JavaTextClassLibrary"/>
		<rdfs:subClassOf rdf:resource="&java;JavaClassLibrary"/>
		<rdfs:comment xml:lang="en">JavaLibrary implementing the java.text package for JDK 1.1</rdfs:comment>
		<rdfs:comment xml:lang="OWLManchester">platform:implementsInterface some JavaTextAPI</rdfs:comment>
	</owl:Class>
	<owl:Class rdf:about="#JavaTextResourcesClassLibrary">
		<rdfs:subClassOf rdf:resource="&personaljava-1_1;JavaTextResourcesClassLibrary"/>
		<rdfs:comment xml:lang="en">JavaLibrary implementing the java.text.resources package for JDK 1.1</rdfs:comment>
		<rdfs:comment xml:lang="OWLManchester">platform:implementsInterface some JavaTextResourcesAPI</rdfs:comment>
	</owl:Class>
	<owl:Class rdf:about="#JavaMathClassLibrary">
		<rdfs:subClassOf rdf:resource="&java;JavaClassLibrary"/>
		<rdfs:comment xml:lang="en">JavaLibrary implementing the java.math package for JDK 1.1</rdfs:comment>
		<rdfs:comment xml:lang="OWLManchester">platform:implementsInterface some JavaMathAPI</rdfs:comment>
	</owl:Class>
	<owl:Class rdf:about="#JavaSecurityClassLibrary">
		<rdfs:subClassOf rdf:resource="&java;JavaClassLibrary"/>
		<rdfs:comment xml:lang="en">JavaLibrary implementing the java.security package for JDK 1.1</rdfs:comment>
		<rdfs:comment xml:lang="OWLManchester">platform:implementsInterface some JavaSecurityAPI</rdfs:comment>
	</owl:Class>
	<owl:Class rdf:about="#JavaSecurityAclClassLibrary">
		<rdfs:subClassOf rdf:resource="&java;JavaClassLibrary"/>
		<rdfs:comment xml:lang="en">JavaLibrary implementing the java.security.acl package for JDK 1.1</rdfs:comment>
		<rdfs:comment xml:lang="OWLManchester">platform:implementsInterface some JavaSecurityAclAPI</rdfs:comment>
	</owl:Class>
	<owl:Class rdf:about="#JavaSecurityInterfacesClassLibrary">
		<rdfs:subClassOf rdf:resource="&java;JavaClassLibrary"/>
		<rdfs:comment xml:lang="en">JavaLibrary implementing the java.security.interfaces package for JDK 1.1</rdfs:comment>
		<rdfs:comment xml:lang="OWLManchester">platform:implementsInterface some JavaSecurityInterfacesAPI</rdfs:comment>
	</owl:Class>
	<owl:Class rdf:about="#JavaAwtClassLibrary">
		<rdfs:subClassOf rdf:resource="&personaljava-1_1;JavaAwtClassLibrary"/>
		<rdfs:comment xml:lang="en">JavaLibrary implementing the java.awt package for JDK 1.1</rdfs:comment>
		<rdfs:comment xml:lang="OWLManchester">platform:implementsInterface some JavaAwtAPI</rdfs:comment>
	</owl:Class>
	<owl:Class rdf:about="#JavaAwtImageClassLibrary">
		<owl:equivalentClass rdf:resource="&personaljava-1_1;JavaAwtImageClassLibrary"/>
		<rdfs:subClassOf rdf:resource="&java;JavaClassLibrary"/>
		<rdfs:comment xml:lang="en">JavaLibrary implementing the java.awt.image package for JDK 1.1</rdfs:comment>
		<rdfs:comment xml:lang="OWLManchester">platform:implementsInterface some JavaAwtImageAPI</rdfs:comment>
	</owl:Class>
	<owl:Class rdf:about="#JavaAwtDatatransferClassLibrary">
		<owl:equivalentClass rdf:resource="&personaljava-1_1;JavaAwtDatatransferClassLibrary"/>
		<rdfs:subClassOf rdf:resource="&java;JavaClassLibrary"/>
		<rdfs:comment xml:lang="en">JavaLibrary implementing the java.awt.datatransfer package for JDK 1.1</rdfs:comment>
		<rdfs:comment xml:lang="OWLManchester">platform:implementsInterface some JavaAwtDatatransferAPI</rdfs:comment>
	</owl:Class>
	<owl:Class rdf:about="#JavaAwtEventClassLibrary">
		<owl:equivalentClass rdf:resource="&personaljava-1_1;JavaAwtEventClassLibrary"/>
		<rdfs:subClassOf rdf:resource="&java;JavaClassLibrary"/>
		<rdfs:comment xml:lang="en">JavaLibrary implementing the java.awt.event package for JDK 1.1</rdfs:comment>
		<rdfs:comment xml:lang="OWLManchester">platform:implementsInterface some JavaAwtEventAPI</rdfs:comment>
	</owl:Class>
	<owl:Class rdf:about="#JavaAppletClassLibrary">
		<owl:equivalentClass rdf:resource="&personaljava-1_1;JavaAppletClassLibrary"/>
		<rdfs:subClassOf rdf:resource="&java;JavaClassLibrary"/>
		<rdfs:comment xml:lang="en">JavaLibrary implementing the java.applet package for JDK 1.1</rdfs:comment>
		<rdfs:comment xml:lang="OWLManchester">platform:implementsInterface some JavaAppletAPI</rdfs:comment>
	</owl:Class>
	<owl:Class rdf:about="#JavaSqlClassLibrary">
		<rdfs:subClassOf rdf:resource="&java;JavaClassLibrary"/>
		<rdfs:comment xml:lang="en">JavaLibrary implementing the java.sql package for JDK 1.1</rdfs:comment>
		<rdfs:comment xml:lang="OWLManchester">platform:implementsInterface some JavaSqlAPI</rdfs:comment>
	</owl:Class>
	<owl:Class rdf:about="#JavaRmiClassLibrary">
		<rdfs:subClassOf rdf:resource="&java;JavaClassLibrary"/>
		<rdfs:comment xml:lang="en">JavaLibrary implementing the java.rmi package for JDK 1.1</rdfs:comment>
		<rdfs:comment xml:lang="OWLManchester">platform:implementsInterface some JavaRmiAPI</rdfs:comment>
	</owl:Class>
	<owl:Class rdf:about="#JavaRmiRegistryClassLibrary">
		<rdfs:subClassOf rdf:resource="&java;JavaClassLibrary"/>
		<rdfs:comment xml:lang="en">JavaLibrary implementing the java.rmi.registry package for JDK 1.1</rdfs:comment>
		<rdfs:comment xml:lang="OWLManchester">platform:implementsInterface some JavaRmiRegistryAPI</rdfs:comment>
	</owl:Class>
	<owl:Class rdf:about="#JavaRmiDgcClassLibrary">
		<rdfs:subClassOf rdf:resource="&java;JavaClassLibrary"/>
		<rdfs:comment xml:lang="en">JavaLibrary implementing the java.rmi.dgc package for JDK 1.1</rdfs:comment>
		<rdfs:comment xml:lang="OWLManchester">platform:implementsInterface some JavaRmiDgcAPI</rdfs:comment>
	</owl:Class>
	<owl:Class rdf:about="#JavaRmiServerClassLibrary">
		<rdfs:subClassOf rdf:resource="&java;JavaClassLibrary"/>
		<rdfs:comment xml:lang="en">JavaLibrary implementing the java.rmi.server package for JDK 1.1</rdfs:comment>
		<rdfs:comment xml:lang="OWLManchester">platform:implementsInterface some JavaRmiServerAPI</rdfs:comment>
	</owl:Class>
	<owl:Class rdf:about="#JavaBeansClassLibrary">
		<owl:equivalentClass rdf:resource="&personaljava-1_1;JavaBeansClassLibrary"/>
		<rdfs:subClassOf rdf:resource="&java;JavaClassLibrary"/>
		<rdfs:comment xml:lang="en">JavaLibrary implementing the java.beans package for JDK 1.1</rdfs:comment>
		<rdfs:comment xml:lang="OWLManchester">platform:implementsInterface some JavaBeansAPI</rdfs:comment>
	</owl:Class>
</rdf:RDF>
