<?xml version="1.0"?>


<!DOCTYPE rdf:RDF [
    <!ENTITY owl "http://www.w3.org/2002/07/owl#" >
    <!ENTITY dc "http://purl.org/dc/elements/1.1/" >
    <!ENTITY xsd "http://www.w3.org/2001/XMLSchema#" >
    <!ENTITY owl2xml "http://www.w3.org/2006/12/owl2-xml#" >
    <!ENTITY rdfs "http://www.w3.org/2000/01/rdf-schema#" >
    <!ENTITY rdf "http://www.w3.org/1999/02/22-rdf-syntax-ns#" >
    <!ENTITY isa "http://soft.vub.ac.be/platformkit/2010/1/isa.owl#" >
    <!ENTITY arm "http://soft.vub.ac.be/platformkit/2010/1/arm.owl#" >
]>


<rdf:RDF xmlns="http://soft.vub.ac.be/platformkit/2010/1/arm.owl#"
     xml:base="http://soft.vub.ac.be/platformkit/2010/1/arm.owl"
     xmlns:dc="http://purl.org/dc/elements/1.1/"
     xmlns:rdfs="http://www.w3.org/2000/01/rdf-schema#"
     xmlns:owl2xml="http://www.w3.org/2006/12/owl2-xml#"
     xmlns:isa="http://soft.vub.ac.be/platformkit/2010/1/isa.owl#"
     xmlns:owl="http://www.w3.org/2002/07/owl#"
     xmlns:xsd="http://www.w3.org/2001/XMLSchema#"
     xmlns:rdf="http://www.w3.org/1999/02/22-rdf-syntax-ns#"
     xmlns:arm="http://soft.vub.ac.be/platformkit/2010/1/arm.owl#">
    <owl:Ontology rdf:about="">
        <rdfs:label xml:lang="en"
            >PlatformKit ARM instruction set architecture ontology.</rdfs:label>
        <dc:creator
            >Dennis Wagelaar &lt;dennis.wagelaar@vub.ac.be&gt;</dc:creator>
        <owl:versionInfo>$Id$</owl:versionInfo>
        <rdfs:comment xml:lang="en"
            >Describes and disambiguates the different ARM instruction set architectures.</rdfs:comment>
        <dc:rights xml:lang="en"
            >&#169; 2010, Vrije Universiteit Brussel. All rights reserved.</dc:rights>
        <owl:imports rdf:resource="http://soft.vub.ac.be/platformkit/2010/1/isa.owl"/>
    </owl:Ontology>
    


    <!-- 
    ///////////////////////////////////////////////////////////////////////////////////////
    //
    // Annotation properties
    //
    ///////////////////////////////////////////////////////////////////////////////////////
     -->

    <owl:AnnotationProperty rdf:about="&dc;creator"/>
    <owl:AnnotationProperty rdf:about="&dc;rights"/>
    


    <!-- 
    ///////////////////////////////////////////////////////////////////////////////////////
    //
    // Classes
    //
    ///////////////////////////////////////////////////////////////////////////////////////
     -->

    


    <!-- http://soft.vub.ac.be/platformkit/2010/1/arm.owl#ARMv1 -->

    <owl:Class rdf:about="#ARMv1">
        <rdfs:subClassOf rdf:resource="&isa;ARM"/>
        <rdfs:comment xml:lang="en"
            >ARMv1 (obsolete).</rdfs:comment>
        <rdfs:seeAlso
            >http://en.wikipedia.org/wiki/ARM_architecture#Instruction_set</rdfs:seeAlso>
    </owl:Class>
    


    <!-- http://soft.vub.ac.be/platformkit/2010/1/arm.owl#ARMv2 -->

    <owl:Class rdf:about="#ARMv2">
        <rdfs:subClassOf rdf:resource="#ARMv1"/>
        <rdfs:seeAlso
            >http://en.wikipedia.org/wiki/ARM_architecture#Instruction_set</rdfs:seeAlso>
        <rdfs:comment xml:lang="en"
            >ARMv2 (obsolete). Architecture 2 added the MUL (multiply) instruction.</rdfs:comment>
    </owl:Class>
    


    <!-- http://soft.vub.ac.be/platformkit/2010/1/arm.owl#ARMv2a -->

    <owl:Class rdf:about="#ARMv2a">
        <rdfs:subClassOf rdf:resource="#ARMv2"/>
        <rdfs:seeAlso
            >http://en.wikipedia.org/wiki/ARM_architecture#Instruction_set</rdfs:seeAlso>
        <rdfs:comment xml:lang="en"
            >ARMv2a (obsolete). Architecture 2a added the SWP and SWPB (swap) instructions.</rdfs:comment>
    </owl:Class>
    


    <!-- http://soft.vub.ac.be/platformkit/2010/1/arm.owl#ARMv3 -->

    <owl:Class rdf:about="#ARMv3">
        <rdfs:subClassOf rdf:resource="#ARMv2a"/>
        <rdfs:comment xml:lang="en"
            >ARMv3 (obsolete). v3 architecture first to support addressing 32 bits of memory (as opposed to 26 bits).</rdfs:comment>
        <rdfs:seeAlso
            >http://en.wikipedia.org/wiki/ARM_architecture#Instruction_set</rdfs:seeAlso>
    </owl:Class>
    


    <!-- http://soft.vub.ac.be/platformkit/2010/1/arm.owl#ARMv4 -->

    <owl:Class rdf:about="#ARMv4">
        <rdfs:subClassOf rdf:resource="#ARMv3"/>
        <rdfs:comment xml:lang="en"
            >ARMv4 (StrongARM).</rdfs:comment>
        <rdfs:seeAlso
            >http://en.wikipedia.org/wiki/ARM_architecture#Instruction_set</rdfs:seeAlso>
    </owl:Class>
    


    <!-- http://soft.vub.ac.be/platformkit/2010/1/arm.owl#ARMv4T -->

    <owl:Class rdf:about="#ARMv4T">
        <rdfs:subClassOf rdf:resource="#ARMv4"/>
        <rdfs:comment xml:lang="en">ARMv4T. Thumb.</rdfs:comment>
        <rdfs:seeAlso
            >http://en.wikipedia.org/wiki/ARM_architecture#Instruction_set</rdfs:seeAlso>
    </owl:Class>
    


    <!-- http://soft.vub.ac.be/platformkit/2010/1/arm.owl#ARMv5TE -->

    <owl:Class rdf:about="#ARMv5TE">
        <rdfs:subClassOf rdf:resource="#ARMv4T"/>
        <rdfs:comment xml:lang="en"
            >ARMv5TE. Thumb, Enhanced DSP instructions.</rdfs:comment>
        <rdfs:seeAlso
            >http://en.wikipedia.org/wiki/ARM_architecture#Instruction_set</rdfs:seeAlso>
    </owl:Class>
    


    <!-- http://soft.vub.ac.be/platformkit/2010/1/arm.owl#ARMv5TEJ -->

    <owl:Class rdf:about="#ARMv5TEJ">
        <rdfs:subClassOf rdf:resource="#ARMv5TE"/>
        <rdfs:comment xml:lang="en"
            >ARMv5TEJ. Thumb, Jazelle DBX, Enhanced DSP instructions.</rdfs:comment>
        <rdfs:seeAlso
            >http://en.wikipedia.org/wiki/ARM_architecture#Instruction_set</rdfs:seeAlso>
    </owl:Class>
    


    <!-- http://soft.vub.ac.be/platformkit/2010/1/arm.owl#ARMv6 -->

    <owl:Class rdf:about="#ARMv6">
        <rdfs:subClassOf rdf:resource="#ARMv5TEJ"/>
        <rdfs:subClassOf rdf:resource="#ARMv6-M"/>
        <rdfs:comment xml:lang="en"
            >ARMv6. SIMD, Thumb, Jazelle DBX, (VFP), Enhanced DSP instructions.</rdfs:comment>
        <rdfs:seeAlso
            >http://en.wikipedia.org/wiki/ARM_architecture#Instruction_set</rdfs:seeAlso>
    </owl:Class>
    


    <!-- http://soft.vub.ac.be/platformkit/2010/1/arm.owl#ARMv6-M -->

    <owl:Class rdf:about="#ARMv6-M">
        <rdfs:subClassOf rdf:resource="#ARMv5TE"/>
        <rdfs:seeAlso
            >http://en.wikipedia.org/wiki/ARM_architecture#Instruction_set</rdfs:seeAlso>
        <rdfs:comment xml:lang="en"
            >ARMv6-M. Microcontroller profile, Thumb-2 subset (16-bit Thumb instructions &amp; BL, MRS, MSR, ISB, DSB, and DMB).</rdfs:comment>
    </owl:Class>
    


    <!-- http://soft.vub.ac.be/platformkit/2010/1/arm.owl#ARMv6K -->

    <owl:Class rdf:about="#ARMv6K">
        <rdfs:subClassOf rdf:resource="#ARMv6"/>
        <rdfs:comment xml:lang="en"
            >ARMv6K. SIMD, Thumb, Jazelle DBX, (VFP), Enhanced DSP instructions, 1&#8211;4 core SMP.</rdfs:comment>
        <rdfs:seeAlso
            >http://en.wikipedia.org/wiki/ARM_architecture#Instruction_set</rdfs:seeAlso>
    </owl:Class>
    


    <!-- http://soft.vub.ac.be/platformkit/2010/1/arm.owl#ARMv6KZ -->

    <owl:Class rdf:about="#ARMv6KZ">
        <rdfs:subClassOf rdf:resource="#ARMv6"/>
        <rdfs:comment xml:lang="en"
            >ARMv6KZ. SIMD, Thumb, Jazelle DBX, (VFP), Enhanced DSP instructions.</rdfs:comment>
        <rdfs:seeAlso
            >http://en.wikipedia.org/wiki/ARM_architecture#Instruction_set</rdfs:seeAlso>
    </owl:Class>
    


    <!-- http://soft.vub.ac.be/platformkit/2010/1/arm.owl#ARMv6T2 -->

    <owl:Class rdf:about="#ARMv6T2">
        <rdfs:subClassOf rdf:resource="#ARMv6-M"/>
        <rdfs:seeAlso
            >http://en.wikipedia.org/wiki/ARM_architecture#Instruction_set</rdfs:seeAlso>
        <rdfs:comment xml:lang="en"
            >ARMv6T2. SIMD, Thumb-2, (VFP), Enhanced DSP instructions.</rdfs:comment>
    </owl:Class>
    


    <!-- http://soft.vub.ac.be/platformkit/2010/1/arm.owl#ARMv7-A -->

    <owl:Class rdf:about="#ARMv7-A">
        <rdfs:subClassOf rdf:resource="#ARMv6T2"/>
        <rdfs:subClassOf rdf:resource="#ARMv7-R"/>
        <rdfs:comment xml:lang="en"
            >ARMv7-A. Application profile, VFP, NEON, Jazelle RCT, Thumb-2.</rdfs:comment>
        <rdfs:seeAlso
            >http://en.wikipedia.org/wiki/ARM_architecture#Instruction_set</rdfs:seeAlso>
    </owl:Class>
    


    <!-- http://soft.vub.ac.be/platformkit/2010/1/arm.owl#ARMv7-M -->

    <owl:Class rdf:about="#ARMv7-M">
        <rdfs:subClassOf rdf:resource="#ARMv6-M"/>
        <rdfs:seeAlso
            >http://en.wikipedia.org/wiki/ARM_architecture#Instruction_set</rdfs:seeAlso>
        <rdfs:comment xml:lang="en"
            >ARMv7-M. Microcontroller profile, Thumb-2 only. Hardware divide instruction.</rdfs:comment>
    </owl:Class>
    


    <!-- http://soft.vub.ac.be/platformkit/2010/1/arm.owl#ARMv7-R -->

    <owl:Class rdf:about="#ARMv7-R">
        <rdfs:subClassOf rdf:resource="#ARMv7-M"/>
        <rdfs:comment xml:lang="en"
            >ARMv7-R. Embedded profile, Thumb-2, (FPU).</rdfs:comment>
        <rdfs:seeAlso
            >http://en.wikipedia.org/wiki/ARM_architecture#Instruction_set</rdfs:seeAlso>
    </owl:Class>
    


    <!-- http://soft.vub.ac.be/platformkit/2010/1/isa.owl#ARM -->

    <owl:Class rdf:about="&isa;ARM"/>
</rdf:RDF>



<!-- Generated by the OWL API (version 2.2.1.1138) http://owlapi.sourceforge.net -->

