<?xml version="1.0"?>


<!DOCTYPE rdf:RDF [
    <!ENTITY owl "http://www.w3.org/2002/07/owl#" >
    <!ENTITY dc "http://purl.org/dc/elements/1.1/" >
    <!ENTITY xsd "http://www.w3.org/2001/XMLSchema#" >
    <!ENTITY owl2xml "http://www.w3.org/2006/12/owl2-xml#" >
    <!ENTITY rdfs "http://www.w3.org/2000/01/rdf-schema#" >
    <!ENTITY rdf "http://www.w3.org/1999/02/22-rdf-syntax-ns#" >
    <!ENTITY platform "http://soft.vub.ac.be/platformkit/2010/1/platform.owl#" >
]>


<rdf:RDF xmlns="http://soft.vub.ac.be/platformkit/2010/1/platform.owl#"
     xml:base="http://soft.vub.ac.be/platformkit/2010/1/platform.owl"
     xmlns:dc="http://purl.org/dc/elements/1.1/"
     xmlns:platform="http://soft.vub.ac.be/platformkit/2010/1/platform.owl#"
     xmlns:rdfs="http://www.w3.org/2000/01/rdf-schema#"
     xmlns:owl2xml="http://www.w3.org/2006/12/owl2-xml#"
     xmlns:owl="http://www.w3.org/2002/07/owl#"
     xmlns:xsd="http://www.w3.org/2001/XMLSchema#"
     xmlns:rdf="http://www.w3.org/1999/02/22-rdf-syntax-ns#">
    <owl:Ontology rdf:about="">
        <rdfs:label xml:lang="en"
            >PlatformKit root platform ontology.</rdfs:label>
        <owl:versionInfo rdf:datatype="&xsd;string"
            >$Id$</owl:versionInfo>
        <dc:creator
            >Dennis Wagelaar &lt;dennis.wagelaar@vub.ac.be&gt;</dc:creator>
        <rdfs:comment xml:lang="en"
            >Platform concepts and definitions.</rdfs:comment>
        <dc:rights xml:lang="en"
            >&#169; 2010, Vrije Universiteit Brussel. All rights reserved.</dc:rights>
    </owl:Ontology>
    


    <!-- 
    ///////////////////////////////////////////////////////////////////////////////////////
    //
    // Annotation properties
    //
    ///////////////////////////////////////////////////////////////////////////////////////
     -->

    <owl:AnnotationProperty rdf:about="&dc;creator"/>
    <owl:AnnotationProperty rdf:about="&dc;rights"/>
    


    <!-- 
    ///////////////////////////////////////////////////////////////////////////////////////
    //
    // Object Properties
    //
    ///////////////////////////////////////////////////////////////////////////////////////
     -->

    


    <!-- http://soft.vub.ac.be/platformkit/2010/1/platform.owl#comprisesInterfacePart -->

    <owl:ObjectProperty rdf:about="#comprisesInterfacePart">
        <rdfs:comment xml:lang="en"
            >The parts that make up a feature interface.</rdfs:comment>
        <rdfs:domain rdf:resource="#FeatureInterface"/>
        <rdfs:range rdf:resource="#FeatureInterfacePart"/>
    </owl:ObjectProperty>
    


    <!-- http://soft.vub.ac.be/platformkit/2010/1/platform.owl#implementsInterface -->

    <owl:ObjectProperty rdf:about="#implementsInterface">
        <rdfs:comment xml:lang="en"
            >The interfaces implemented by the feature.</rdfs:comment>
        <rdfs:domain rdf:resource="#Feature"/>
        <rdfs:range rdf:resource="#FeatureInterface"/>
    </owl:ObjectProperty>
    


    <!-- http://soft.vub.ac.be/platformkit/2010/1/platform.owl#providesFeature -->

    <owl:ObjectProperty rdf:about="#providesFeature">
        <rdfs:comment xml:lang="en"
            >The features (directly) provided or contained by the platform.</rdfs:comment>
        <rdfs:range rdf:resource="#Feature"/>
        <rdfs:domain rdf:resource="#Platform"/>
    </owl:ObjectProperty>
    


    <!-- 
    ///////////////////////////////////////////////////////////////////////////////////////
    //
    // Classes
    //
    ///////////////////////////////////////////////////////////////////////////////////////
     -->

    


    <!-- http://soft.vub.ac.be/platformkit/2010/1/platform.owl#ABI -->

    <owl:Class rdf:about="#ABI">
        <rdfs:subClassOf rdf:resource="#FeatureInterface"/>
        <rdfs:subClassOf>
            <owl:Restriction>
                <owl:onProperty rdf:resource="#comprisesInterfacePart"/>
                <owl:allValuesFrom rdf:resource="#ABIPart"/>
            </owl:Restriction>
        </rdfs:subClassOf>
        <owl:disjointWith rdf:resource="#API"/>
        <rdfs:comment xml:lang="en"
            >An Application Binary Interface is a lower level definition concerning details at the assembly language level.</rdfs:comment>
        <rdfs:seeAlso
            >http://en.wikipedia.org/wiki/Application_binary_interface</rdfs:seeAlso>
    </owl:Class>
    


    <!-- http://soft.vub.ac.be/platformkit/2010/1/platform.owl#ABIPart -->

    <owl:Class rdf:about="#ABIPart">
        <rdfs:subClassOf rdf:resource="#FeatureInterfacePart"/>
        <owl:disjointWith rdf:resource="#APIPart"/>
        <rdfs:seeAlso
            >http://en.wikipedia.org/wiki/Application_binary_interface</rdfs:seeAlso>
        <rdfs:comment xml:lang="en"
            >Part of an ABI. Allows for partitioning of ABIs for the purpose of defining partial platform dependency constraints.</rdfs:comment>
    </owl:Class>
    


    <!-- http://soft.vub.ac.be/platformkit/2010/1/platform.owl#API -->

    <owl:Class rdf:about="#API">
        <rdfs:subClassOf rdf:resource="#FeatureInterface"/>
        <rdfs:subClassOf>
            <owl:Restriction>
                <owl:onProperty rdf:resource="#comprisesInterfacePart"/>
                <owl:allValuesFrom rdf:resource="#APIPart"/>
            </owl:Restriction>
        </rdfs:subClassOf>
        <rdfs:comment xml:lang="en"
            >An Application Programming Interface provides a programming interface for software. APIs are implemented by software applications, libraries, operating systems, etc.</rdfs:comment>
        <rdfs:seeAlso
            >http://en.wikipedia.org/wiki/Application_programming_interface</rdfs:seeAlso>
    </owl:Class>
    


    <!-- http://soft.vub.ac.be/platformkit/2010/1/platform.owl#APIPart -->

    <owl:Class rdf:about="#APIPart">
        <rdfs:subClassOf rdf:resource="#FeatureInterfacePart"/>
        <rdfs:seeAlso
            >http://en.wikipedia.org/wiki/Application_programming_interface</rdfs:seeAlso>
        <rdfs:comment xml:lang="en"
            >Part of an API. Allows for partitioning of APIs for the purpose of defining partial platform dependency constraints.</rdfs:comment>
    </owl:Class>
    


    <!-- http://soft.vub.ac.be/platformkit/2010/1/platform.owl#Application -->

    <owl:Class rdf:about="#Application">
        <rdfs:subClassOf rdf:resource="#Software"/>
        <rdfs:subClassOf>
            <owl:Restriction>
                <owl:onProperty rdf:resource="#implementsInterface"/>
                <owl:allValuesFrom rdf:resource="#API"/>
            </owl:Restriction>
        </rdfs:subClassOf>
        <rdfs:seeAlso
            >http://en.wikipedia.org/wiki/Application_software</rdfs:seeAlso>
        <rdfs:comment xml:lang="en"
            >Software application, program, or executable.</rdfs:comment>
    </owl:Class>
    


    <!-- http://soft.vub.ac.be/platformkit/2010/1/platform.owl#EABI -->

    <owl:Class rdf:about="#EABI">
        <rdfs:subClassOf rdf:resource="#ISA"/>
        <rdfs:seeAlso
            >http://en.wikipedia.org/wiki/Application_binary_interface</rdfs:seeAlso>
        <rdfs:comment xml:lang="en"
            >Embedded Application Binary Interface. Augments an Instruction Set Architecture with standard bus/memory specifications. Examples are ARM and PowerPC.</rdfs:comment>
    </owl:Class>
    


    <!-- http://soft.vub.ac.be/platformkit/2010/1/platform.owl#Feature -->

    <owl:Class rdf:about="#Feature">
        <owl:disjointWith rdf:resource="#FeatureInterface"/>
        <owl:disjointWith rdf:resource="#FeatureInterfacePart"/>
        <rdfs:comment xml:lang="en"
            >Platform feature. Can be implemented in software or hardware.</rdfs:comment>
    </owl:Class>
    


    <!-- http://soft.vub.ac.be/platformkit/2010/1/platform.owl#FeatureInterface -->

    <owl:Class rdf:about="#FeatureInterface">
        <owl:disjointWith rdf:resource="#FeatureInterfacePart"/>
        <owl:disjointWith rdf:resource="#Platform"/>
        <rdfs:comment xml:lang="en"
            >An interface implemented by a feature, which can be used by other features.</rdfs:comment>
        <rdfs:seeAlso
            >http://en.wikipedia.org/wiki/Interface_%28computer_science%29</rdfs:seeAlso>
    </owl:Class>
    


    <!-- http://soft.vub.ac.be/platformkit/2010/1/platform.owl#FeatureInterfacePart -->

    <owl:Class rdf:about="#FeatureInterfacePart">
        <owl:disjointWith rdf:resource="#Platform"/>
        <rdfs:seeAlso
            >http://en.wikipedia.org/wiki/Interface_%28computer_science%29</rdfs:seeAlso>
        <rdfs:comment xml:lang="en"
            >Part of a feature interface. Allows for partitioning of feature interfaces for the purpose of defining partial platform dependency constraints.</rdfs:comment>
    </owl:Class>
    


    <!-- http://soft.vub.ac.be/platformkit/2010/1/platform.owl#Framework -->

    <owl:Class rdf:about="#Framework">
        <rdfs:subClassOf rdf:resource="#Software"/>
        <rdfs:subClassOf>
            <owl:Restriction>
                <owl:onProperty rdf:resource="#implementsInterface"/>
                <owl:allValuesFrom rdf:resource="#API"/>
            </owl:Restriction>
        </rdfs:subClassOf>
        <rdfs:seeAlso
            >http://en.wikipedia.org/wiki/Software_framework</rdfs:seeAlso>
        <rdfs:comment xml:lang="en"
            >Software framework. Typically implements an API.</rdfs:comment>
    </owl:Class>
    


    <!-- http://soft.vub.ac.be/platformkit/2010/1/platform.owl#Hardware -->

    <owl:Class rdf:about="#Hardware">
        <rdfs:subClassOf rdf:resource="#Feature"/>
        <owl:disjointWith rdf:resource="#Software"/>
        <rdfs:comment xml:lang="en"
            >Platform feature that is implemented in hardware.</rdfs:comment>
        <rdfs:seeAlso
            >http://en.wikipedia.org/wiki/Electronics</rdfs:seeAlso>
    </owl:Class>
    


    <!-- http://soft.vub.ac.be/platformkit/2010/1/platform.owl#IODevice -->

    <owl:Class rdf:about="#IODevice">
        <rdfs:subClassOf rdf:resource="#Hardware"/>
        <rdfs:subClassOf rdf:resource="#IOFeature"/>
        <owl:disjointWith rdf:resource="#Resource"/>
        <rdfs:seeAlso
            >http://en.wikipedia.org/wiki/Input/output</rdfs:seeAlso>
        <rdfs:comment xml:lang="en"
            >Input/output device. Implemented in hardware.</rdfs:comment>
    </owl:Class>
    


    <!-- http://soft.vub.ac.be/platformkit/2010/1/platform.owl#IOFeature -->

    <owl:Class rdf:about="#IOFeature">
        <rdfs:subClassOf rdf:resource="#Feature"/>
        <rdfs:comment xml:lang="en"
            >Input/output feature. Can be implemented in hardware or software.</rdfs:comment>
        <rdfs:seeAlso
            >http://en.wikipedia.org/wiki/Input/output</rdfs:seeAlso>
    </owl:Class>
    


    <!-- http://soft.vub.ac.be/platformkit/2010/1/platform.owl#ISA -->

    <owl:Class rdf:about="#ISA">
        <rdfs:subClassOf rdf:resource="#ABI"/>
        <rdfs:comment xml:lang="en"
            >Instruction Set Architecture of a machine. Can be implemented in hardware or a software virtual machine.</rdfs:comment>
        <rdfs:seeAlso
            >http://en.wikipedia.org/wiki/Category:Instruction_set_architectures</rdfs:seeAlso>
        <rdfs:seeAlso
            >http://en.wikipedia.org/wiki/Instruction_set</rdfs:seeAlso>
    </owl:Class>
    


    <!-- http://soft.vub.ac.be/platformkit/2010/1/platform.owl#Installer -->

    <owl:Class rdf:about="#Installer">
        <rdfs:subClassOf rdf:resource="#Software"/>
        <rdfs:comment xml:lang="en"
            >Software package installer.</rdfs:comment>
        <rdfs:seeAlso
            >http://en.wikipedia.org/wiki/Installer</rdfs:seeAlso>
    </owl:Class>
    


    <!-- http://soft.vub.ac.be/platformkit/2010/1/platform.owl#Library -->

    <owl:Class rdf:about="#Library">
        <rdfs:subClassOf rdf:resource="#Software"/>
        <rdfs:subClassOf>
            <owl:Restriction>
                <owl:onProperty rdf:resource="#implementsInterface"/>
                <owl:allValuesFrom rdf:resource="#API"/>
            </owl:Restriction>
        </rdfs:subClassOf>
        <rdfs:seeAlso
            >http://en.wikipedia.org/wiki/Library_%28computing%29</rdfs:seeAlso>
        <rdfs:comment xml:lang="en"
            >Shared (runtime) software library. Typically implements an API.</rdfs:comment>
    </owl:Class>
    


    <!-- http://soft.vub.ac.be/platformkit/2010/1/platform.owl#OperatingSystem -->

    <owl:Class rdf:about="#OperatingSystem">
        <rdfs:subClassOf rdf:resource="#Platform"/>
        <rdfs:subClassOf rdf:resource="#Software"/>
        <rdfs:seeAlso
            >http://en.wikipedia.org/wiki/Operating_system</rdfs:seeAlso>
        <rdfs:comment xml:lang="en"
            >Computer operating system.</rdfs:comment>
    </owl:Class>
    


    <!-- http://soft.vub.ac.be/platformkit/2010/1/platform.owl#PackageManager -->

    <owl:Class rdf:about="#PackageManager">
        <rdfs:subClassOf rdf:resource="#Installer"/>
        <rdfs:comment xml:lang="en"
            >Software package manager. Manages installation and dependencies of software packages.</rdfs:comment>
        <rdfs:seeAlso
            >http://en.wikipedia.org/wiki/Package_manager</rdfs:seeAlso>
    </owl:Class>
    


    <!-- http://soft.vub.ac.be/platformkit/2010/1/platform.owl#Platform -->

    <owl:Class rdf:about="#Platform">
        <rdfs:comment xml:lang="en"
            >Combination of hardware and/or software features on top of which new features can be built.</rdfs:comment>
        <rdfs:seeAlso
            >http://en.wikipedia.org/wiki/Computing_platform</rdfs:seeAlso>
    </owl:Class>
    


    <!-- http://soft.vub.ac.be/platformkit/2010/1/platform.owl#Resource -->

    <owl:Class rdf:about="#Resource">
        <rdfs:subClassOf rdf:resource="#Hardware"/>
        <rdfs:comment xml:lang="en"
            >Quantifiable hardware resource, providing a certain amount of, e.g. processing power, memory, etc.</rdfs:comment>
        <rdfs:seeAlso
            >http://en.wikipedia.org/wiki/Resource_%28computer_science%29</rdfs:seeAlso>
    </owl:Class>
    


    <!-- http://soft.vub.ac.be/platformkit/2010/1/platform.owl#RuntimeEnvironment -->

    <owl:Class rdf:about="#RuntimeEnvironment">
        <rdfs:subClassOf rdf:resource="#Platform"/>
        <rdfs:subClassOf rdf:resource="#Software"/>
        <rdfs:comment xml:lang="en"
            >Software runtime environment.</rdfs:comment>
        <rdfs:seeAlso
            >http://en.wikipedia.org/wiki/Runtime_environment</rdfs:seeAlso>
    </owl:Class>
    


    <!-- http://soft.vub.ac.be/platformkit/2010/1/platform.owl#Software -->

    <owl:Class rdf:about="#Software">
        <rdfs:subClassOf rdf:resource="#Feature"/>
        <rdfs:seeAlso
            >http://en.wikipedia.org/wiki/Software</rdfs:seeAlso>
        <rdfs:comment xml:lang="en"
            >Platform feature that is implemented in software.</rdfs:comment>
    </owl:Class>
    


    <!-- http://soft.vub.ac.be/platformkit/2010/1/platform.owl#VirtualIODevice -->

    <owl:Class rdf:about="#VirtualIODevice">
        <rdfs:subClassOf rdf:resource="#IOFeature"/>
        <rdfs:subClassOf rdf:resource="#Software"/>
        <rdfs:seeAlso
            >http://en.wikipedia.org/wiki/Virtual_keyboard</rdfs:seeAlso>
        <rdfs:comment xml:lang="en"
            >Virtual input/output device that is implemented in software.</rdfs:comment>
    </owl:Class>
    


    <!-- http://soft.vub.ac.be/platformkit/2010/1/platform.owl#VirtualMachine -->

    <owl:Class rdf:about="#VirtualMachine">
        <rdfs:subClassOf rdf:resource="#Software"/>
        <rdfs:subClassOf>
            <owl:Restriction>
                <owl:onProperty rdf:resource="#implementsInterface"/>
                <owl:allValuesFrom rdf:resource="#ISA"/>
            </owl:Restriction>
        </rdfs:subClassOf>
        <rdfs:comment xml:lang="en"
            >Software virtual machine. Typically implements an instruction set architecture.</rdfs:comment>
        <rdfs:seeAlso
            >http://en.wikipedia.org/wiki/Virtual_machine</rdfs:seeAlso>
    </owl:Class>
    


    <!-- 
    ///////////////////////////////////////////////////////////////////////////////////////
    //
    // General axioms
    //
    ///////////////////////////////////////////////////////////////////////////////////////
     -->

    <rdf:Description>
        <rdf:type rdf:resource="&owl;AllDisjointClasses"/>
        <owl:members rdf:parseType="Collection">
            <rdf:Description rdf:about="#Application"/>
            <rdf:Description rdf:about="#Framework"/>
            <rdf:Description rdf:about="#Installer"/>
            <rdf:Description rdf:about="#Library"/>
            <rdf:Description rdf:about="#OperatingSystem"/>
            <rdf:Description rdf:about="#RuntimeEnvironment"/>
            <rdf:Description rdf:about="#VirtualIODevice"/>
            <rdf:Description rdf:about="#VirtualMachine"/>
        </owl:members>
    </rdf:Description>
</rdf:RDF>



<!-- Generated by the OWL API (version 2.2.1.1138) http://owlapi.sourceforge.net -->

