<?xml version="1.0" encoding="ISO-8859-1"?>
<!DOCTYPE rdf:RDF [
	<!ENTITY xsd "http://www.w3.org/2001/XMLSchema#">
	<!ENTITY owl "http://www.w3.org/2002/07/owl#">
	<!ENTITY rdfs "http://www.w3.org/2000/01/rdf-schema#">
	<!ENTITY rdf "http://www.w3.org/1999/02/22-rdf-syntax-ns#">
	<!ENTITY units "http://www.cs.kuleuven.be/~distrinet/projects/CoDAMoS/2005/01/Units.owl#">
	<!ENTITY platform "http://www.cs.kuleuven.be/~distrinet/projects/CoDAMoS/2007/01/Platform.owl#">
	<!ENTITY java "http://ssel.vub.ac.be/codamos/2007/01/Java.owl#">
	<!ENTITY j2se-1_4 "http://ssel.vub.ac.be/codamos/2007/01/j2se-1_4-api.owl#">
	<!ENTITY DEFAULT "http://ssel.vub.ac.be/codamos/2007/01/j2se-1_5-api.owl">
]>
<rdf:RDF
	 xmlns:xsd="&xsd;"
	 xmlns:owl="&owl;"
	 xmlns:rdfs="&rdfs;"
	 xmlns:rdf="&rdf;"
	 xmlns:units="&units;"
	 xmlns:platform="&platform;"
	 xmlns:java="&java;"
	 xmlns:j2se-1_4="&j2se-1_4;"
	 xmlns = "&DEFAULT;#"
	 xml:base = "&DEFAULT;"
>

	<owl:Ontology rdf:about="">
		<owl:imports rdf:resource="http://www.cs.kuleuven.be/~distrinet/projects/CoDAMoS/2007/01/Platform.owl"/>
		<owl:imports rdf:resource="http://ssel.vub.ac.be/codamos/2007/01/Java.owl"/>
		<owl:imports rdf:resource="http://ssel.vub.ac.be/codamos/2007/01/j2se-1_4-api.owl"/>
		<rdfs:comment xml:lang="en">Generated by $Id: UML2ToPackageAPIOntology.atl 6906 2007-06-14 11:28:36Z dwagelaa $ and $Id: UML2ToAPIOntology.atl 6906 2007-06-14 11:28:36Z dwagelaa $</rdfs:comment>
		<rdfs:label xml:lang="en">j2se-1_5</rdfs:label>
	</owl:Ontology>
	<owl:Class rdf:about="#J2se-1_5ClassLibrary">
		<rdfs:subClassOf rdf:resource="#JavaAppletLibrary"/>
		<rdfs:subClassOf rdf:resource="#JavaAwtLibrary"/>
		<rdfs:subClassOf rdf:resource="#JavaAwtEventLibrary"/>
		<rdfs:subClassOf rdf:resource="#JavaAwtImageLibrary"/>
		<rdfs:subClassOf rdf:resource="#JavaAwtImageRenderableLibrary"/>
		<rdfs:subClassOf rdf:resource="#JavaAwtColorLibrary"/>
		<rdfs:subClassOf rdf:resource="#JavaAwtDatatransferLibrary"/>
		<rdfs:subClassOf rdf:resource="#JavaAwtDndLibrary"/>
		<rdfs:subClassOf rdf:resource="#JavaAwtDndPeerLibrary"/>
		<rdfs:subClassOf rdf:resource="#JavaAwtFontLibrary"/>
		<rdfs:subClassOf rdf:resource="#JavaAwtGeomLibrary"/>
		<rdfs:subClassOf rdf:resource="#JavaAwtImLibrary"/>
		<rdfs:subClassOf rdf:resource="#JavaAwtImSpiLibrary"/>
		<rdfs:subClassOf rdf:resource="#JavaAwtPeerLibrary"/>
		<rdfs:subClassOf rdf:resource="#JavaAwtPrintLibrary"/>
		<rdfs:subClassOf rdf:resource="#JavaLangLibrary"/>
		<rdfs:subClassOf rdf:resource="#JavaLangReflectLibrary"/>
		<rdfs:subClassOf rdf:resource="#JavaLangAnnotationLibrary"/>
		<rdfs:subClassOf rdf:resource="#JavaLangInstrumentLibrary"/>
		<rdfs:subClassOf rdf:resource="#JavaLangManagementLibrary"/>
		<rdfs:subClassOf rdf:resource="#JavaLangRefLibrary"/>
		<rdfs:subClassOf rdf:resource="#JavaSecurityLibrary"/>
		<rdfs:subClassOf rdf:resource="#JavaSecurityAclLibrary"/>
		<rdfs:subClassOf rdf:resource="#JavaSecurityCertLibrary"/>
		<rdfs:subClassOf rdf:resource="#JavaSecurityInterfacesLibrary"/>
		<rdfs:subClassOf rdf:resource="#JavaSecuritySpecLibrary"/>
		<rdfs:subClassOf rdf:resource="#JavaIoLibrary"/>
		<rdfs:subClassOf rdf:resource="#JavaUtilLibrary"/>
		<rdfs:subClassOf rdf:resource="#JavaUtilConcurrentLibrary"/>
		<rdfs:subClassOf rdf:resource="#JavaUtilConcurrentAtomicLibrary"/>
		<rdfs:subClassOf rdf:resource="#JavaUtilConcurrentLocksLibrary"/>
		<rdfs:subClassOf rdf:resource="#JavaUtilJarLibrary"/>
		<rdfs:subClassOf rdf:resource="#JavaUtilZipLibrary"/>
		<rdfs:subClassOf rdf:resource="#JavaUtilLoggingLibrary"/>
		<rdfs:subClassOf rdf:resource="#JavaUtilPrefsLibrary"/>
		<rdfs:subClassOf rdf:resource="#JavaUtilRegexLibrary"/>
		<rdfs:subClassOf rdf:resource="#JavaBeansLibrary"/>
		<rdfs:subClassOf rdf:resource="#JavaBeansBeancontextLibrary"/>
		<rdfs:subClassOf rdf:resource="#JavaMathLibrary"/>
		<rdfs:subClassOf rdf:resource="#JavaNetLibrary"/>
		<rdfs:subClassOf rdf:resource="#JavaNioLibrary"/>
		<rdfs:subClassOf rdf:resource="#JavaNioChannelsLibrary"/>
		<rdfs:subClassOf rdf:resource="#JavaNioChannelsSpiLibrary"/>
		<rdfs:subClassOf rdf:resource="#JavaNioCharsetLibrary"/>
		<rdfs:subClassOf rdf:resource="#JavaNioCharsetSpiLibrary"/>
		<rdfs:subClassOf rdf:resource="#JavaRmiLibrary"/>
		<rdfs:subClassOf rdf:resource="#JavaRmiActivationLibrary"/>
		<rdfs:subClassOf rdf:resource="#JavaRmiServerLibrary"/>
		<rdfs:subClassOf rdf:resource="#JavaRmiDgcLibrary"/>
		<rdfs:subClassOf rdf:resource="#JavaRmiRegistryLibrary"/>
		<rdfs:subClassOf rdf:resource="#JavaSqlLibrary"/>
		<rdfs:subClassOf rdf:resource="#JavaTextLibrary"/>
		<rdfs:subClassOf rdf:resource="#JavaxAccessibilityLibrary"/>
		<rdfs:subClassOf rdf:resource="#JavaxSecurityAuthLibrary"/>
		<rdfs:subClassOf rdf:resource="#JavaxSecurityAuthCallbackLibrary"/>
		<rdfs:subClassOf rdf:resource="#JavaxSecurityAuthKerberosLibrary"/>
		<rdfs:subClassOf rdf:resource="#JavaxSecurityAuthLoginLibrary"/>
		<rdfs:subClassOf rdf:resource="#JavaxSecurityAuthSpiLibrary"/>
		<rdfs:subClassOf rdf:resource="#JavaxSecurityAuthX500Library"/>
		<rdfs:subClassOf rdf:resource="#JavaxSecuritySaslLibrary"/>
		<rdfs:subClassOf rdf:resource="#JavaxActivityLibrary"/>
		<rdfs:subClassOf rdf:resource="#JavaxImageioLibrary"/>
		<rdfs:subClassOf rdf:resource="#JavaxImageioEventLibrary"/>
		<rdfs:subClassOf rdf:resource="#JavaxImageioMetadataLibrary"/>
		<rdfs:subClassOf rdf:resource="#JavaxImageioPluginsBmpLibrary"/>
		<rdfs:subClassOf rdf:resource="#JavaxImageioPluginsJpegLibrary"/>
		<rdfs:subClassOf rdf:resource="#JavaxImageioSpiLibrary"/>
		<rdfs:subClassOf rdf:resource="#JavaxImageioStreamLibrary"/>
		<rdfs:subClassOf rdf:resource="#JavaxManagementLibrary"/>
		<rdfs:subClassOf rdf:resource="#JavaxManagementLoadingLibrary"/>
		<rdfs:subClassOf rdf:resource="#JavaxManagementModelmbeanLibrary"/>
		<rdfs:subClassOf rdf:resource="#JavaxManagementMonitorLibrary"/>
		<rdfs:subClassOf rdf:resource="#JavaxManagementOpenmbeanLibrary"/>
		<rdfs:subClassOf rdf:resource="#JavaxManagementRelationLibrary"/>
		<rdfs:subClassOf rdf:resource="#JavaxManagementRemoteLibrary"/>
		<rdfs:subClassOf rdf:resource="#JavaxManagementRemoteRmiLibrary"/>
		<rdfs:subClassOf rdf:resource="#JavaxManagementTimerLibrary"/>
		<rdfs:subClassOf rdf:resource="#JavaxNamingLibrary"/>
		<rdfs:subClassOf rdf:resource="#JavaxNamingDirectoryLibrary"/>
		<rdfs:subClassOf rdf:resource="#JavaxNamingEventLibrary"/>
		<rdfs:subClassOf rdf:resource="#JavaxNamingLdapLibrary"/>
		<rdfs:subClassOf rdf:resource="#JavaxNamingSpiLibrary"/>
		<rdfs:subClassOf rdf:resource="#JavaxPrintLibrary"/>
		<rdfs:subClassOf rdf:resource="#JavaxPrintAttributeLibrary"/>
		<rdfs:subClassOf rdf:resource="#JavaxPrintAttributeStandardLibrary"/>
		<rdfs:subClassOf rdf:resource="#JavaxPrintEventLibrary"/>
		<rdfs:subClassOf rdf:resource="#JavaxRmiLibrary"/>
		<rdfs:subClassOf rdf:resource="#JavaxRmiCORBALibrary"/>
		<rdfs:subClassOf rdf:resource="#JavaxRmiSslLibrary"/>
		<rdfs:subClassOf rdf:resource="#JavaxCryptoLibrary"/>
		<rdfs:subClassOf rdf:resource="#JavaxSoundMidiLibrary"/>
		<rdfs:subClassOf rdf:resource="#JavaxSoundMidiSpiLibrary"/>
		<rdfs:subClassOf rdf:resource="#JavaxSoundSampledLibrary"/>
		<rdfs:subClassOf rdf:resource="#JavaxSoundSampledSpiLibrary"/>
		<rdfs:subClassOf rdf:resource="#JavaxSqlLibrary"/>
		<rdfs:subClassOf rdf:resource="#JavaxSqlRowsetLibrary"/>
		<rdfs:subClassOf rdf:resource="#JavaxSqlRowsetSerialLibrary"/>
		<rdfs:subClassOf rdf:resource="#JavaxSqlRowsetSpiLibrary"/>
		<rdfs:subClassOf rdf:resource="#JavaxSwingLibrary"/>
		<rdfs:subClassOf rdf:resource="#JavaxSwingTextLibrary"/>
		<rdfs:subClassOf rdf:resource="#JavaxSwingTextHtmlLibrary"/>
		<rdfs:subClassOf rdf:resource="#JavaxSwingTextHtmlParserLibrary"/>
		<rdfs:subClassOf rdf:resource="#JavaxSwingTextRtfLibrary"/>
		<rdfs:subClassOf rdf:resource="#JavaxSwingEventLibrary"/>
		<rdfs:subClassOf rdf:resource="#JavaxSwingTreeLibrary"/>
		<rdfs:subClassOf rdf:resource="#JavaxSwingBorderLibrary"/>
		<rdfs:subClassOf rdf:resource="#JavaxSwingColorchooserLibrary"/>
		<rdfs:subClassOf rdf:resource="#JavaxSwingFilechooserLibrary"/>
		<rdfs:subClassOf rdf:resource="#JavaxSwingPlafLibrary"/>
		<rdfs:subClassOf rdf:resource="#JavaxSwingPlafBasicLibrary"/>
		<rdfs:subClassOf rdf:resource="#JavaxSwingPlafMetalLibrary"/>
		<rdfs:subClassOf rdf:resource="#JavaxSwingPlafMultiLibrary"/>
		<rdfs:subClassOf rdf:resource="#JavaxSwingPlafSynthLibrary"/>
		<rdfs:subClassOf rdf:resource="#JavaxSwingTableLibrary"/>
		<rdfs:subClassOf rdf:resource="#JavaxSwingUndoLibrary"/>
		<rdfs:subClassOf rdf:resource="#JavaxTransactionLibrary"/>
		<rdfs:subClassOf rdf:resource="#JavaxTransactionXaLibrary"/>
		<rdfs:subClassOf rdf:resource="#JavaxXmlLibrary"/>
		<rdfs:subClassOf rdf:resource="#JavaxXmlDatatypeLibrary"/>
		<rdfs:subClassOf rdf:resource="#JavaxXmlNamespaceLibrary"/>
		<rdfs:subClassOf rdf:resource="#JavaxXmlParsersLibrary"/>
		<rdfs:subClassOf rdf:resource="#JavaxXmlTransformLibrary"/>
		<rdfs:subClassOf rdf:resource="#JavaxXmlTransformDomLibrary"/>
		<rdfs:subClassOf rdf:resource="#JavaxXmlTransformSaxLibrary"/>
		<rdfs:subClassOf rdf:resource="#JavaxXmlTransformStreamLibrary"/>
		<rdfs:subClassOf rdf:resource="#JavaxXmlValidationLibrary"/>
		<rdfs:subClassOf rdf:resource="#JavaxXmlXpathLibrary"/>
		<rdfs:subClassOf rdf:resource="#OrgW3cDomLibrary"/>
		<rdfs:subClassOf rdf:resource="#OrgW3cDomBootstrapLibrary"/>
		<rdfs:subClassOf rdf:resource="#OrgW3cDomCssLibrary"/>
		<rdfs:subClassOf rdf:resource="#OrgW3cDomStylesheetsLibrary"/>
		<rdfs:subClassOf rdf:resource="#OrgW3cDomViewsLibrary"/>
		<rdfs:subClassOf rdf:resource="#OrgW3cDomEventsLibrary"/>
		<rdfs:subClassOf rdf:resource="#OrgW3cDomHtmlLibrary"/>
		<rdfs:subClassOf rdf:resource="#OrgW3cDomLsLibrary"/>
		<rdfs:subClassOf rdf:resource="#OrgW3cDomTraversalLibrary"/>
		<rdfs:subClassOf rdf:resource="#OrgW3cDomRangesLibrary"/>
		<rdfs:subClassOf rdf:resource="#OrgOmgCORBA_2_3Library"/>
		<rdfs:subClassOf rdf:resource="#OrgOmgCORBA_2_3PortableLibrary"/>
		<rdfs:subClassOf rdf:resource="#OrgOmgCORBALibrary"/>
		<rdfs:subClassOf rdf:resource="#OrgOmgCORBAPortableLibrary"/>
		<rdfs:subClassOf rdf:resource="#OrgOmgCORBADynAnyPackageLibrary"/>
		<rdfs:subClassOf rdf:resource="#OrgOmgCORBAORBPackageLibrary"/>
		<rdfs:subClassOf rdf:resource="#OrgOmgCORBATypeCodePackageLibrary"/>
		<rdfs:subClassOf rdf:resource="#OrgOmgCosNamingLibrary"/>
		<rdfs:subClassOf rdf:resource="#OrgOmgCosNamingNamingContextExtPackageLibrary"/>
		<rdfs:subClassOf rdf:resource="#OrgOmgCosNamingNamingContextPackageLibrary"/>
		<rdfs:subClassOf rdf:resource="#OrgOmgPortableServerLibrary"/>
		<rdfs:subClassOf rdf:resource="#OrgOmgPortableServerCurrentPackageLibrary"/>
		<rdfs:subClassOf rdf:resource="#OrgOmgPortableServerPOAManagerPackageLibrary"/>
		<rdfs:subClassOf rdf:resource="#OrgOmgPortableServerPOAPackageLibrary"/>
		<rdfs:subClassOf rdf:resource="#OrgOmgPortableServerServantLocatorPackageLibrary"/>
		<rdfs:subClassOf rdf:resource="#OrgOmgPortableServerPortableLibrary"/>
		<rdfs:subClassOf rdf:resource="#OrgOmgDynamicLibrary"/>
		<rdfs:subClassOf rdf:resource="#OrgOmgDynamicAnyLibrary"/>
		<rdfs:subClassOf rdf:resource="#OrgOmgDynamicAnyDynAnyFactoryPackageLibrary"/>
		<rdfs:subClassOf rdf:resource="#OrgOmgDynamicAnyDynAnyPackageLibrary"/>
		<rdfs:subClassOf rdf:resource="#OrgOmgIOPLibrary"/>
		<rdfs:subClassOf rdf:resource="#OrgOmgIOPCodecFactoryPackageLibrary"/>
		<rdfs:subClassOf rdf:resource="#OrgOmgIOPCodecPackageLibrary"/>
		<rdfs:subClassOf rdf:resource="#OrgOmgMessagingLibrary"/>
		<rdfs:subClassOf rdf:resource="#OrgOmgPortableInterceptorLibrary"/>
		<rdfs:subClassOf rdf:resource="#OrgOmgPortableInterceptorORBInitInfoPackageLibrary"/>
		<rdfs:subClassOf rdf:resource="#OrgOmgSendingContextLibrary"/>
		<rdfs:subClassOf rdf:resource="#OrgOmgStubJavaRmiLibrary"/>
		<rdfs:subClassOf rdf:resource="#OrgOmgStubJavaxManagementRemoteRmiLibrary"/>
		<rdfs:subClassOf rdf:resource="#OrgXmlSaxLibrary"/>
		<rdfs:subClassOf rdf:resource="#OrgXmlSaxExtLibrary"/>
		<rdfs:subClassOf rdf:resource="#OrgXmlSaxHelpersLibrary"/>
		<rdfs:subClassOf rdf:resource="#OrgIetfJgssLibrary"/>
		<rdfs:comment xml:lang="en">JavaLibrary implementing the entire API for j2se-1_5</rdfs:comment>
	</owl:Class>
	<owl:Class rdf:about="#J2se-1_5">
		<rdfs:subClassOf rdf:resource="&java;JRE"/>
		<rdfs:subClassOf>
			<owl:Restriction>
				<owl:onProperty rdf:resource="&java;providesBuiltinJavaLibrary"/>
				<owl:someValuesFrom rdf:resource="#J2se-1_5ClassLibrary"/>
			</owl:Restriction>
		</rdfs:subClassOf>
		<rdfs:comment xml:lang="en">j2se-1_5 Java Runtime Environment</rdfs:comment>
	</owl:Class>
	<owl:Class rdf:about="#JavaAppletLibrary">
		<rdfs:subClassOf rdf:resource="&j2se-1_4;JavaAppletLibrary"/>
		<rdfs:seeAlso rdf:resource="#JavaUtilLibrary"/>
		<rdfs:seeAlso rdf:resource="#JavaLangLibrary"/>
		<rdfs:seeAlso rdf:resource="#JavaxAccessibilityLibrary"/>
		<rdfs:seeAlso rdf:resource="#JavaNetLibrary"/>
		<rdfs:seeAlso rdf:resource="#JavaIoLibrary"/>
		<rdfs:seeAlso rdf:resource="#JavaAwtLibrary"/>
		<rdfs:comment xml:lang="en">JavaLibrary implementing the java.applet package for j2se-1_5</rdfs:comment>
	</owl:Class>
	<owl:Class rdf:about="#JavaAwtLibrary">
		<rdfs:subClassOf rdf:resource="&j2se-1_4;JavaAwtLibrary"/>
		<rdfs:seeAlso rdf:resource="#JavaxAccessibilityLibrary"/>
		<rdfs:seeAlso rdf:resource="#JavaAwtDndPeerLibrary"/>
		<rdfs:seeAlso rdf:resource="#JavaUtilLibrary"/>
		<rdfs:seeAlso rdf:resource="#JavaAwtGeomLibrary"/>
		<rdfs:seeAlso rdf:resource="#JavaTextLibrary"/>
		<rdfs:seeAlso rdf:resource="#JavaIoLibrary"/>
		<rdfs:seeAlso rdf:resource="#JavaLangLibrary"/>
		<rdfs:seeAlso rdf:resource="#JavaxSwingTextLibrary"/>
		<rdfs:seeAlso rdf:resource="#JavaNetLibrary"/>
		<rdfs:seeAlso rdf:resource="#JavaAwtDatatransferLibrary"/>
		<rdfs:seeAlso rdf:resource="#JavaAwtEventLibrary"/>
		<rdfs:seeAlso rdf:resource="#JavaSecurityLibrary"/>
		<rdfs:seeAlso rdf:resource="#JavaAwtImageLibrary"/>
		<rdfs:seeAlso rdf:resource="#JavaAwtPeerLibrary"/>
		<rdfs:seeAlso rdf:resource="#JavaAwtColorLibrary"/>
		<rdfs:seeAlso rdf:resource="#JavaBeansLibrary"/>
		<rdfs:seeAlso rdf:resource="#JavaAwtDndLibrary"/>
		<rdfs:seeAlso rdf:resource="#JavaAwtFontLibrary"/>
		<rdfs:seeAlso rdf:resource="#JavaAwtImageRenderableLibrary"/>
		<rdfs:seeAlso rdf:resource="#JavaAwtImLibrary"/>
		<rdfs:comment xml:lang="en">JavaLibrary implementing the java.awt package for j2se-1_5</rdfs:comment>
	</owl:Class>
	<owl:Class rdf:about="#JavaAwtEventLibrary">
		<rdfs:subClassOf rdf:resource="&j2se-1_4;JavaAwtEventLibrary"/>
		<rdfs:seeAlso rdf:resource="#JavaUtilLibrary"/>
		<rdfs:seeAlso rdf:resource="#JavaLangLibrary"/>
		<rdfs:seeAlso rdf:resource="#JavaAwtFontLibrary"/>
		<rdfs:seeAlso rdf:resource="#JavaAwtLibrary"/>
		<rdfs:seeAlso rdf:resource="#JavaTextLibrary"/>
		<rdfs:comment xml:lang="en">JavaLibrary implementing the java.awt.event package for j2se-1_5</rdfs:comment>
	</owl:Class>
	<owl:Class rdf:about="#JavaAwtImageLibrary">
		<rdfs:subClassOf rdf:resource="&j2se-1_4;JavaAwtImageLibrary"/>
		<rdfs:seeAlso rdf:resource="#JavaMathLibrary"/>
		<rdfs:seeAlso rdf:resource="#JavaAwtColorLibrary"/>
		<rdfs:seeAlso rdf:resource="#JavaUtilLibrary"/>
		<rdfs:seeAlso rdf:resource="#JavaLangLibrary"/>
		<rdfs:seeAlso rdf:resource="#JavaAwtGeomLibrary"/>
		<rdfs:seeAlso rdf:resource="#JavaAwtLibrary"/>
		<rdfs:comment xml:lang="en">JavaLibrary implementing the java.awt.image package for j2se-1_5</rdfs:comment>
	</owl:Class>
	<owl:Class rdf:about="#JavaAwtImageRenderableLibrary">
		<owl:equivalentClass rdf:resource="&j2se-1_4;JavaAwtImageRenderableLibrary"/>
		<rdfs:subClassOf rdf:resource="&java;JavaLibrary"/>
		<rdfs:seeAlso rdf:resource="#JavaUtilLibrary"/>
		<rdfs:seeAlso rdf:resource="#JavaLangLibrary"/>
		<rdfs:seeAlso rdf:resource="#JavaIoLibrary"/>
		<rdfs:seeAlso rdf:resource="#JavaAwtGeomLibrary"/>
		<rdfs:seeAlso rdf:resource="#JavaAwtLibrary"/>
		<rdfs:seeAlso rdf:resource="#JavaAwtImageLibrary"/>
		<rdfs:comment xml:lang="en">JavaLibrary implementing the java.awt.image.renderable package for j2se-1_5</rdfs:comment>
	</owl:Class>
	<owl:Class rdf:about="#JavaAwtColorLibrary">
		<rdfs:subClassOf rdf:resource="&j2se-1_4;JavaAwtColorLibrary"/>
		<rdfs:seeAlso rdf:resource="#JavaIoLibrary"/>
		<rdfs:seeAlso rdf:resource="#JavaLangLibrary"/>
		<rdfs:comment xml:lang="en">JavaLibrary implementing the java.awt.color package for j2se-1_5</rdfs:comment>
	</owl:Class>
	<owl:Class rdf:about="#JavaAwtDatatransferLibrary">
		<rdfs:subClassOf rdf:resource="&j2se-1_4;JavaAwtDatatransferLibrary"/>
		<rdfs:seeAlso rdf:resource="#JavaUtilLibrary"/>
		<rdfs:seeAlso rdf:resource="#JavaLangLibrary"/>
		<rdfs:seeAlso rdf:resource="#JavaIoLibrary"/>
		<rdfs:comment xml:lang="en">JavaLibrary implementing the java.awt.datatransfer package for j2se-1_5</rdfs:comment>
	</owl:Class>
	<owl:Class rdf:about="#JavaAwtDndLibrary">
		<rdfs:subClassOf rdf:resource="&j2se-1_4;JavaAwtDndLibrary"/>
		<rdfs:seeAlso rdf:resource="#JavaIoLibrary"/>
		<rdfs:seeAlso rdf:resource="#JavaAwtLibrary"/>
		<rdfs:seeAlso rdf:resource="#JavaAwtEventLibrary"/>
		<rdfs:seeAlso rdf:resource="#JavaAwtDatatransferLibrary"/>
		<rdfs:seeAlso rdf:resource="#JavaAwtPeerLibrary"/>
		<rdfs:seeAlso rdf:resource="#JavaAwtDndPeerLibrary"/>
		<rdfs:seeAlso rdf:resource="#JavaUtilLibrary"/>
		<rdfs:seeAlso rdf:resource="#JavaLangLibrary"/>
		<rdfs:comment xml:lang="en">JavaLibrary implementing the java.awt.dnd package for j2se-1_5</rdfs:comment>
	</owl:Class>
	<owl:Class rdf:about="#JavaAwtDndPeerLibrary">
		<owl:equivalentClass rdf:resource="&j2se-1_4;JavaAwtDndPeerLibrary"/>
		<rdfs:subClassOf rdf:resource="&java;JavaLibrary"/>
		<rdfs:seeAlso rdf:resource="#JavaAwtDndLibrary"/>
		<rdfs:seeAlso rdf:resource="#JavaAwtLibrary"/>
		<rdfs:seeAlso rdf:resource="#JavaAwtDatatransferLibrary"/>
		<rdfs:comment xml:lang="en">JavaLibrary implementing the java.awt.dnd.peer package for j2se-1_5</rdfs:comment>
	</owl:Class>
	<owl:Class rdf:about="#JavaAwtFontLibrary">
		<owl:equivalentClass rdf:resource="&j2se-1_4;JavaAwtFontLibrary"/>
		<rdfs:subClassOf rdf:resource="&java;JavaLibrary"/>
		<rdfs:seeAlso rdf:resource="#JavaUtilLibrary"/>
		<rdfs:seeAlso rdf:resource="#JavaLangLibrary"/>
		<rdfs:seeAlso rdf:resource="#JavaIoLibrary"/>
		<rdfs:seeAlso rdf:resource="#JavaAwtGeomLibrary"/>
		<rdfs:seeAlso rdf:resource="#JavaAwtLibrary"/>
		<rdfs:seeAlso rdf:resource="#JavaTextLibrary"/>
		<rdfs:comment xml:lang="en">JavaLibrary implementing the java.awt.font package for j2se-1_5</rdfs:comment>
	</owl:Class>
	<owl:Class rdf:about="#JavaAwtGeomLibrary">
		<owl:equivalentClass rdf:resource="&j2se-1_4;JavaAwtGeomLibrary"/>
		<rdfs:subClassOf rdf:resource="&java;JavaLibrary"/>
		<rdfs:seeAlso rdf:resource="#JavaIoLibrary"/>
		<rdfs:seeAlso rdf:resource="#JavaLangLibrary"/>
		<rdfs:seeAlso rdf:resource="#JavaAwtLibrary"/>
		<rdfs:comment xml:lang="en">JavaLibrary implementing the java.awt.geom package for j2se-1_5</rdfs:comment>
	</owl:Class>
	<owl:Class rdf:about="#JavaAwtImLibrary">
		<owl:equivalentClass rdf:resource="&j2se-1_4;JavaAwtImLibrary"/>
		<rdfs:subClassOf rdf:resource="&java;JavaLibrary"/>
		<rdfs:seeAlso rdf:resource="#JavaUtilLibrary"/>
		<rdfs:seeAlso rdf:resource="#JavaLangLibrary"/>
		<rdfs:seeAlso rdf:resource="#JavaAwtFontLibrary"/>
		<rdfs:seeAlso rdf:resource="#JavaAwtLibrary"/>
		<rdfs:seeAlso rdf:resource="#JavaTextLibrary"/>
		<rdfs:comment xml:lang="en">JavaLibrary implementing the java.awt.im package for j2se-1_5</rdfs:comment>
	</owl:Class>
	<owl:Class rdf:about="#JavaAwtImSpiLibrary">
		<owl:equivalentClass rdf:resource="&j2se-1_4;JavaAwtImSpiLibrary"/>
		<rdfs:subClassOf rdf:resource="&java;JavaLibrary"/>
		<rdfs:seeAlso rdf:resource="#JavaUtilLibrary"/>
		<rdfs:seeAlso rdf:resource="#JavaLangLibrary"/>
		<rdfs:seeAlso rdf:resource="#JavaAwtImLibrary"/>
		<rdfs:seeAlso rdf:resource="#JavaxSwingLibrary"/>
		<rdfs:seeAlso rdf:resource="#JavaAwtFontLibrary"/>
		<rdfs:seeAlso rdf:resource="#JavaAwtLibrary"/>
		<rdfs:seeAlso rdf:resource="#JavaTextLibrary"/>
		<rdfs:comment xml:lang="en">JavaLibrary implementing the java.awt.im.spi package for j2se-1_5</rdfs:comment>
	</owl:Class>
	<owl:Class rdf:about="#JavaAwtPeerLibrary">
		<rdfs:subClassOf rdf:resource="&java;JavaLibrary"/>
		<rdfs:seeAlso rdf:resource="#JavaIoLibrary"/>
		<rdfs:seeAlso rdf:resource="#JavaAwtLibrary"/>
		<rdfs:seeAlso rdf:resource="#JavaAwtEventLibrary"/>
		<rdfs:seeAlso rdf:resource="#JavaAwtImageLibrary"/>
		<rdfs:seeAlso rdf:resource="#JavaLangLibrary"/>
		<rdfs:seeAlso rdf:resource="#JavaAwtImLibrary"/>
		<rdfs:comment xml:lang="en">JavaLibrary implementing the java.awt.peer package for j2se-1_5</rdfs:comment>
	</owl:Class>
	<owl:Class rdf:about="#JavaAwtPrintLibrary">
		<owl:equivalentClass rdf:resource="&j2se-1_4;JavaAwtPrintLibrary"/>
		<rdfs:subClassOf rdf:resource="&java;JavaLibrary"/>
		<rdfs:seeAlso rdf:resource="#JavaIoLibrary"/>
		<rdfs:seeAlso rdf:resource="#JavaLangLibrary"/>
		<rdfs:seeAlso rdf:resource="#JavaxPrintAttributeLibrary"/>
		<rdfs:seeAlso rdf:resource="#JavaxPrintLibrary"/>
		<rdfs:seeAlso rdf:resource="#JavaAwtLibrary"/>
		<rdfs:comment xml:lang="en">JavaLibrary implementing the java.awt.print package for j2se-1_5</rdfs:comment>
	</owl:Class>
	<owl:Class rdf:about="#JavaLangLibrary">
		<rdfs:subClassOf rdf:resource="&java;JavaLibrary"/>
		<rdfs:seeAlso rdf:resource="#JavaNetLibrary"/>
		<rdfs:seeAlso rdf:resource="#JavaIoLibrary"/>
		<rdfs:seeAlso rdf:resource="#JavaSecurityLibrary"/>
		<rdfs:seeAlso rdf:resource="#JavaNioLibrary"/>
		<rdfs:seeAlso rdf:resource="#JavaNioChannelsLibrary"/>
		<rdfs:seeAlso rdf:resource="#JavaUtilLibrary"/>
		<rdfs:seeAlso rdf:resource="#JavaLangAnnotationLibrary"/>
		<rdfs:seeAlso rdf:resource="#JavaLangReflectLibrary"/>
		<rdfs:comment xml:lang="en">JavaLibrary implementing the java.lang package for j2se-1_5</rdfs:comment>
	</owl:Class>
	<owl:Class rdf:about="#JavaLangReflectLibrary">
		<rdfs:subClassOf rdf:resource="&j2se-1_4;JavaLangReflectLibrary"/>
		<rdfs:seeAlso rdf:resource="#JavaIoLibrary"/>
		<rdfs:seeAlso rdf:resource="#JavaSecurityLibrary"/>
		<rdfs:seeAlso rdf:resource="#JavaLangLibrary"/>
		<rdfs:seeAlso rdf:resource="#JavaLangAnnotationLibrary"/>
		<rdfs:comment xml:lang="en">JavaLibrary implementing the java.lang.reflect package for j2se-1_5</rdfs:comment>
	</owl:Class>
	<owl:Class rdf:about="#JavaLangAnnotationLibrary">
		<rdfs:subClassOf rdf:resource="&java;JavaLibrary"/>
		<rdfs:seeAlso rdf:resource="#JavaLangLibrary"/>
		<rdfs:seeAlso rdf:resource="#JavaLangReflectLibrary"/>
		<rdfs:comment xml:lang="en">JavaLibrary implementing the java.lang.annotation package for j2se-1_5</rdfs:comment>
	</owl:Class>
	<owl:Class rdf:about="#JavaLangInstrumentLibrary">
		<rdfs:subClassOf rdf:resource="&java;JavaLibrary"/>
		<rdfs:seeAlso rdf:resource="#JavaLangLibrary"/>
		<rdfs:seeAlso rdf:resource="#JavaSecurityLibrary"/>
		<rdfs:comment xml:lang="en">JavaLibrary implementing the java.lang.instrument package for j2se-1_5</rdfs:comment>
	</owl:Class>
	<owl:Class rdf:about="#JavaLangManagementLibrary">
		<rdfs:subClassOf rdf:resource="&java;JavaLibrary"/>
		<rdfs:seeAlso rdf:resource="#JavaUtilLibrary"/>
		<rdfs:seeAlso rdf:resource="#JavaxManagementOpenmbeanLibrary"/>
		<rdfs:seeAlso rdf:resource="#JavaSecurityLibrary"/>
		<rdfs:seeAlso rdf:resource="#JavaLangLibrary"/>
		<rdfs:seeAlso rdf:resource="#JavaxManagementLibrary"/>
		<rdfs:comment xml:lang="en">JavaLibrary implementing the java.lang.management package for j2se-1_5</rdfs:comment>
	</owl:Class>
	<owl:Class rdf:about="#JavaLangRefLibrary">
		<owl:equivalentClass rdf:resource="&j2se-1_4;JavaLangRefLibrary"/>
		<rdfs:subClassOf rdf:resource="&java;JavaLibrary"/>
		<rdfs:seeAlso rdf:resource="#JavaLangLibrary"/>
		<rdfs:comment xml:lang="en">JavaLibrary implementing the java.lang.ref package for j2se-1_5</rdfs:comment>
	</owl:Class>
	<owl:Class rdf:about="#JavaSecurityLibrary">
		<rdfs:subClassOf rdf:resource="&j2se-1_4;JavaSecurityLibrary"/>
		<rdfs:seeAlso rdf:resource="#JavaxSecurityAuthCallbackLibrary"/>
		<rdfs:seeAlso rdf:resource="#JavaNetLibrary"/>
		<rdfs:seeAlso rdf:resource="#JavaSecurityCertLibrary"/>
		<rdfs:seeAlso rdf:resource="#JavaIoLibrary"/>
		<rdfs:seeAlso rdf:resource="#JavaNioLibrary"/>
		<rdfs:seeAlso rdf:resource="#JavaxSecurityAuthLibrary"/>
		<rdfs:seeAlso rdf:resource="#JavaUtilLibrary"/>
		<rdfs:seeAlso rdf:resource="#JavaLangLibrary"/>
		<rdfs:seeAlso rdf:resource="#JavaSecuritySpecLibrary"/>
		<rdfs:seeAlso rdf:resource="#JavaxCryptoLibrary"/>
		<rdfs:comment xml:lang="en">JavaLibrary implementing the java.security package for j2se-1_5</rdfs:comment>
	</owl:Class>
	<owl:Class rdf:about="#JavaSecurityAclLibrary">
		<owl:equivalentClass rdf:resource="&j2se-1_4;JavaSecurityAclLibrary"/>
		<rdfs:subClassOf rdf:resource="&java;JavaLibrary"/>
		<rdfs:seeAlso rdf:resource="#JavaUtilLibrary"/>
		<rdfs:seeAlso rdf:resource="#JavaLangLibrary"/>
		<rdfs:seeAlso rdf:resource="#JavaSecurityLibrary"/>
		<rdfs:comment xml:lang="en">JavaLibrary implementing the java.security.acl package for j2se-1_5</rdfs:comment>
	</owl:Class>
	<owl:Class rdf:about="#JavaSecurityCertLibrary">
		<rdfs:subClassOf rdf:resource="&j2se-1_4;JavaSecurityCertLibrary"/>
		<rdfs:seeAlso rdf:resource="#JavaMathLibrary"/>
		<rdfs:seeAlso rdf:resource="#JavaUtilLibrary"/>
		<rdfs:seeAlso rdf:resource="#JavaLangLibrary"/>
		<rdfs:seeAlso rdf:resource="#JavaIoLibrary"/>
		<rdfs:seeAlso rdf:resource="#JavaSecurityLibrary"/>
		<rdfs:seeAlso rdf:resource="#JavaxSecurityAuthX500Library"/>
		<rdfs:comment xml:lang="en">JavaLibrary implementing the java.security.cert package for j2se-1_5</rdfs:comment>
	</owl:Class>
	<owl:Class rdf:about="#JavaSecurityInterfacesLibrary">
		<rdfs:subClassOf rdf:resource="&j2se-1_4;JavaSecurityInterfacesLibrary"/>
		<rdfs:seeAlso rdf:resource="#JavaMathLibrary"/>
		<rdfs:seeAlso rdf:resource="#JavaSecurityLibrary"/>
		<rdfs:seeAlso rdf:resource="#JavaSecuritySpecLibrary"/>
		<rdfs:comment xml:lang="en">JavaLibrary implementing the java.security.interfaces package for j2se-1_5</rdfs:comment>
	</owl:Class>
	<owl:Class rdf:about="#JavaSecuritySpecLibrary">
		<rdfs:subClassOf rdf:resource="&j2se-1_4;JavaSecuritySpecLibrary"/>
		<rdfs:seeAlso rdf:resource="#JavaMathLibrary"/>
		<rdfs:seeAlso rdf:resource="#JavaSecurityInterfacesLibrary"/>
		<rdfs:seeAlso rdf:resource="#JavaSecurityLibrary"/>
		<rdfs:seeAlso rdf:resource="#JavaLangLibrary"/>
		<rdfs:comment xml:lang="en">JavaLibrary implementing the java.security.spec package for j2se-1_5</rdfs:comment>
	</owl:Class>
	<owl:Class rdf:about="#JavaIoLibrary">
		<rdfs:subClassOf rdf:resource="&j2se-1_4;JavaIoLibrary"/>
		<rdfs:seeAlso rdf:resource="#JavaUtilLibrary"/>
		<rdfs:seeAlso rdf:resource="#JavaLangLibrary"/>
		<rdfs:seeAlso rdf:resource="#JavaNetLibrary"/>
		<rdfs:seeAlso rdf:resource="#JavaNioCharsetLibrary"/>
		<rdfs:seeAlso rdf:resource="#JavaSecurityLibrary"/>
		<rdfs:seeAlso rdf:resource="#JavaNioLibrary"/>
		<rdfs:seeAlso rdf:resource="#JavaNioChannelsLibrary"/>
		<rdfs:comment xml:lang="en">JavaLibrary implementing the java.io package for j2se-1_5</rdfs:comment>
	</owl:Class>
	<owl:Class rdf:about="#JavaUtilLibrary">
		<rdfs:subClassOf rdf:resource="&j2se-1_4;JavaUtilLibrary"/>
		<rdfs:seeAlso rdf:resource="#JavaMathLibrary"/>
		<rdfs:seeAlso rdf:resource="#JavaIoLibrary"/>
		<rdfs:seeAlso rdf:resource="#JavaSecurityLibrary"/>
		<rdfs:seeAlso rdf:resource="#JavaNioChannelsLibrary"/>
		<rdfs:seeAlso rdf:resource="#JavaLangLibrary"/>
		<rdfs:seeAlso rdf:resource="#JavaUtilRegexLibrary"/>
		<rdfs:comment xml:lang="en">JavaLibrary implementing the java.util package for j2se-1_5</rdfs:comment>
	</owl:Class>
	<owl:Class rdf:about="#JavaUtilConcurrentLibrary">
		<rdfs:subClassOf rdf:resource="&java;JavaLibrary"/>
		<rdfs:seeAlso rdf:resource="#JavaIoLibrary"/>
		<rdfs:seeAlso rdf:resource="#JavaSecurityLibrary"/>
		<rdfs:seeAlso rdf:resource="#JavaUtilLibrary"/>
		<rdfs:seeAlso rdf:resource="#JavaLangLibrary"/>
		<rdfs:comment xml:lang="en">JavaLibrary implementing the java.util.concurrent package for j2se-1_5</rdfs:comment>
	</owl:Class>
	<owl:Class rdf:about="#JavaUtilConcurrentAtomicLibrary">
		<rdfs:subClassOf rdf:resource="&java;JavaLibrary"/>
		<rdfs:seeAlso rdf:resource="#JavaIoLibrary"/>
		<rdfs:seeAlso rdf:resource="#JavaLangLibrary"/>
		<rdfs:comment xml:lang="en">JavaLibrary implementing the java.util.concurrent.atomic package for j2se-1_5</rdfs:comment>
	</owl:Class>
	<owl:Class rdf:about="#JavaUtilConcurrentLocksLibrary">
		<rdfs:subClassOf rdf:resource="&java;JavaLibrary"/>
		<rdfs:seeAlso rdf:resource="#JavaUtilLibrary"/>
		<rdfs:seeAlso rdf:resource="#JavaIoLibrary"/>
		<rdfs:seeAlso rdf:resource="#JavaLangLibrary"/>
		<rdfs:seeAlso rdf:resource="#JavaUtilConcurrentLibrary"/>
		<rdfs:comment xml:lang="en">JavaLibrary implementing the java.util.concurrent.locks package for j2se-1_5</rdfs:comment>
	</owl:Class>
	<owl:Class rdf:about="#JavaUtilJarLibrary">
		<rdfs:subClassOf rdf:resource="&j2se-1_4;JavaUtilJarLibrary"/>
		<rdfs:seeAlso rdf:resource="#JavaUtilLibrary"/>
		<rdfs:seeAlso rdf:resource="#JavaBeansLibrary"/>
		<rdfs:seeAlso rdf:resource="#JavaLangLibrary"/>
		<rdfs:seeAlso rdf:resource="#JavaIoLibrary"/>
		<rdfs:seeAlso rdf:resource="#JavaUtilZipLibrary"/>
		<rdfs:comment xml:lang="en">JavaLibrary implementing the java.util.jar package for j2se-1_5</rdfs:comment>
	</owl:Class>
	<owl:Class rdf:about="#JavaUtilZipLibrary">
		<rdfs:subClassOf rdf:resource="&j2se-1_4;JavaUtilZipLibrary"/>
		<rdfs:seeAlso rdf:resource="#JavaUtilLibrary"/>
		<rdfs:seeAlso rdf:resource="#JavaIoLibrary"/>
		<rdfs:seeAlso rdf:resource="#JavaLangLibrary"/>
		<rdfs:comment xml:lang="en">JavaLibrary implementing the java.util.zip package for j2se-1_5</rdfs:comment>
	</owl:Class>
	<owl:Class rdf:about="#JavaUtilLoggingLibrary">
		<rdfs:subClassOf rdf:resource="&j2se-1_4;JavaUtilLoggingLibrary"/>
		<rdfs:seeAlso rdf:resource="#JavaUtilLibrary"/>
		<rdfs:seeAlso rdf:resource="#JavaBeansLibrary"/>
		<rdfs:seeAlso rdf:resource="#JavaLangLibrary"/>
		<rdfs:seeAlso rdf:resource="#JavaIoLibrary"/>
		<rdfs:seeAlso rdf:resource="#JavaSecurityLibrary"/>
		<rdfs:comment xml:lang="en">JavaLibrary implementing the java.util.logging package for j2se-1_5</rdfs:comment>
	</owl:Class>
	<owl:Class rdf:about="#JavaUtilPrefsLibrary">
		<owl:equivalentClass rdf:resource="&j2se-1_4;JavaUtilPrefsLibrary"/>
		<rdfs:subClassOf rdf:resource="&java;JavaLibrary"/>
		<rdfs:seeAlso rdf:resource="#JavaIoLibrary"/>
		<rdfs:seeAlso rdf:resource="#JavaUtilLibrary"/>
		<rdfs:seeAlso rdf:resource="#JavaLangLibrary"/>
		<rdfs:comment xml:lang="en">JavaLibrary implementing the java.util.prefs package for j2se-1_5</rdfs:comment>
	</owl:Class>
	<owl:Class rdf:about="#JavaUtilRegexLibrary">
		<rdfs:subClassOf rdf:resource="&j2se-1_4;JavaUtilRegexLibrary"/>
		<rdfs:seeAlso rdf:resource="#JavaIoLibrary"/>
		<rdfs:seeAlso rdf:resource="#JavaLangLibrary"/>
		<rdfs:comment xml:lang="en">JavaLibrary implementing the java.util.regex package for j2se-1_5</rdfs:comment>
	</owl:Class>
	<owl:Class rdf:about="#JavaBeansLibrary">
		<rdfs:subClassOf rdf:resource="&j2se-1_4;JavaBeansLibrary"/>
		<rdfs:seeAlso rdf:resource="#JavaUtilLibrary"/>
		<rdfs:seeAlso rdf:resource="#JavaLangLibrary"/>
		<rdfs:seeAlso rdf:resource="#JavaAppletLibrary"/>
		<rdfs:seeAlso rdf:resource="#JavaBeansBeancontextLibrary"/>
		<rdfs:seeAlso rdf:resource="#JavaIoLibrary"/>
		<rdfs:seeAlso rdf:resource="#JavaAwtLibrary"/>
		<rdfs:seeAlso rdf:resource="#JavaLangReflectLibrary"/>
		<rdfs:comment xml:lang="en">JavaLibrary implementing the java.beans package for j2se-1_5</rdfs:comment>
	</owl:Class>
	<owl:Class rdf:about="#JavaBeansBeancontextLibrary">
		<owl:equivalentClass rdf:resource="&j2se-1_4;JavaBeansBeancontextLibrary"/>
		<rdfs:subClassOf rdf:resource="&java;JavaLibrary"/>
		<rdfs:seeAlso rdf:resource="#JavaNetLibrary"/>
		<rdfs:seeAlso rdf:resource="#JavaIoLibrary"/>
		<rdfs:seeAlso rdf:resource="#JavaAwtLibrary"/>
		<rdfs:seeAlso rdf:resource="#JavaUtilLibrary"/>
		<rdfs:seeAlso rdf:resource="#JavaBeansLibrary"/>
		<rdfs:seeAlso rdf:resource="#JavaLangLibrary"/>
		<rdfs:comment xml:lang="en">JavaLibrary implementing the java.beans.beancontext package for j2se-1_5</rdfs:comment>
	</owl:Class>
	<owl:Class rdf:about="#JavaMathLibrary">
		<rdfs:subClassOf rdf:resource="&j2se-1_4;JavaMathLibrary"/>
		<rdfs:seeAlso rdf:resource="#JavaIoLibrary"/>
		<rdfs:seeAlso rdf:resource="#JavaUtilLibrary"/>
		<rdfs:seeAlso rdf:resource="#JavaLangLibrary"/>
		<rdfs:comment xml:lang="en">JavaLibrary implementing the java.math package for j2se-1_5</rdfs:comment>
	</owl:Class>
	<owl:Class rdf:about="#JavaNetLibrary">
		<rdfs:subClassOf rdf:resource="&j2se-1_4;JavaNetLibrary"/>
		<rdfs:seeAlso rdf:resource="#JavaIoLibrary"/>
		<rdfs:seeAlso rdf:resource="#JavaSecurityLibrary"/>
		<rdfs:seeAlso rdf:resource="#JavaNioChannelsLibrary"/>
		<rdfs:seeAlso rdf:resource="#JavaUtilLibrary"/>
		<rdfs:seeAlso rdf:resource="#JavaUtilJarLibrary"/>
		<rdfs:seeAlso rdf:resource="#JavaLangLibrary"/>
		<rdfs:comment xml:lang="en">JavaLibrary implementing the java.net package for j2se-1_5</rdfs:comment>
	</owl:Class>
	<owl:Class rdf:about="#JavaNioLibrary">
		<rdfs:subClassOf rdf:resource="&j2se-1_4;JavaNioLibrary"/>
		<rdfs:seeAlso rdf:resource="#JavaLangLibrary"/>
		<rdfs:comment xml:lang="en">JavaLibrary implementing the java.nio package for j2se-1_5</rdfs:comment>
	</owl:Class>
	<owl:Class rdf:about="#JavaNioChannelsLibrary">
		<rdfs:subClassOf rdf:resource="&j2se-1_4;JavaNioChannelsLibrary"/>
		<rdfs:seeAlso rdf:resource="#JavaUtilLibrary"/>
		<rdfs:seeAlso rdf:resource="#JavaLangLibrary"/>
		<rdfs:seeAlso rdf:resource="#JavaNetLibrary"/>
		<rdfs:seeAlso rdf:resource="#JavaNioChannelsSpiLibrary"/>
		<rdfs:seeAlso rdf:resource="#JavaIoLibrary"/>
		<rdfs:seeAlso rdf:resource="#JavaNioCharsetLibrary"/>
		<rdfs:seeAlso rdf:resource="#JavaNioLibrary"/>
		<rdfs:comment xml:lang="en">JavaLibrary implementing the java.nio.channels package for j2se-1_5</rdfs:comment>
	</owl:Class>
	<owl:Class rdf:about="#JavaNioChannelsSpiLibrary">
		<rdfs:subClassOf rdf:resource="&j2se-1_4;JavaNioChannelsSpiLibrary"/>
		<rdfs:seeAlso rdf:resource="#JavaUtilLibrary"/>
		<rdfs:seeAlso rdf:resource="#JavaLangLibrary"/>
		<rdfs:seeAlso rdf:resource="#JavaNioChannelsLibrary"/>
		<rdfs:comment xml:lang="en">JavaLibrary implementing the java.nio.channels.spi package for j2se-1_5</rdfs:comment>
	</owl:Class>
	<owl:Class rdf:about="#JavaNioCharsetLibrary">
		<rdfs:subClassOf rdf:resource="&j2se-1_4;JavaNioCharsetLibrary"/>
		<rdfs:seeAlso rdf:resource="#JavaUtilLibrary"/>
		<rdfs:seeAlso rdf:resource="#JavaLangLibrary"/>
		<rdfs:seeAlso rdf:resource="#JavaIoLibrary"/>
		<rdfs:seeAlso rdf:resource="#JavaNioLibrary"/>
		<rdfs:comment xml:lang="en">JavaLibrary implementing the java.nio.charset package for j2se-1_5</rdfs:comment>
	</owl:Class>
	<owl:Class rdf:about="#JavaNioCharsetSpiLibrary">
		<owl:equivalentClass rdf:resource="&j2se-1_4;JavaNioCharsetSpiLibrary"/>
		<rdfs:subClassOf rdf:resource="&java;JavaLibrary"/>
		<rdfs:seeAlso rdf:resource="#JavaUtilLibrary"/>
		<rdfs:seeAlso rdf:resource="#JavaNioCharsetLibrary"/>
		<rdfs:seeAlso rdf:resource="#JavaLangLibrary"/>
		<rdfs:comment xml:lang="en">JavaLibrary implementing the java.nio.charset.spi package for j2se-1_5</rdfs:comment>
	</owl:Class>
	<owl:Class rdf:about="#JavaRmiLibrary">
		<owl:equivalentClass rdf:resource="&j2se-1_4;JavaRmiLibrary"/>
		<rdfs:subClassOf rdf:resource="&java;JavaLibrary"/>
		<rdfs:seeAlso rdf:resource="#JavaIoLibrary"/>
		<rdfs:seeAlso rdf:resource="#JavaLangLibrary"/>
		<rdfs:comment xml:lang="en">JavaLibrary implementing the java.rmi package for j2se-1_5</rdfs:comment>
	</owl:Class>
	<owl:Class rdf:about="#JavaRmiActivationLibrary">
		<owl:equivalentClass rdf:resource="&j2se-1_4;JavaRmiActivationLibrary"/>
		<rdfs:subClassOf rdf:resource="&java;JavaLibrary"/>
		<rdfs:seeAlso rdf:resource="#JavaUtilLibrary"/>
		<rdfs:seeAlso rdf:resource="#JavaLangLibrary"/>
		<rdfs:seeAlso rdf:resource="#JavaRmiLibrary"/>
		<rdfs:seeAlso rdf:resource="#JavaIoLibrary"/>
		<rdfs:seeAlso rdf:resource="#JavaRmiServerLibrary"/>
		<rdfs:comment xml:lang="en">JavaLibrary implementing the java.rmi.activation package for j2se-1_5</rdfs:comment>
	</owl:Class>
	<owl:Class rdf:about="#JavaRmiServerLibrary">
		<rdfs:subClassOf rdf:resource="&j2se-1_4;JavaRmiServerLibrary"/>
		<rdfs:seeAlso rdf:resource="#JavaLangLibrary"/>
		<rdfs:seeAlso rdf:resource="#JavaNetLibrary"/>
		<rdfs:seeAlso rdf:resource="#JavaRmiLibrary"/>
		<rdfs:seeAlso rdf:resource="#JavaIoLibrary"/>
		<rdfs:seeAlso rdf:resource="#JavaLangReflectLibrary"/>
		<rdfs:comment xml:lang="en">JavaLibrary implementing the java.rmi.server package for j2se-1_5</rdfs:comment>
	</owl:Class>
	<owl:Class rdf:about="#JavaRmiDgcLibrary">
		<owl:equivalentClass rdf:resource="&j2se-1_4;JavaRmiDgcLibrary"/>
		<rdfs:subClassOf rdf:resource="&java;JavaLibrary"/>
		<rdfs:seeAlso rdf:resource="#JavaIoLibrary"/>
		<rdfs:seeAlso rdf:resource="#JavaLangLibrary"/>
		<rdfs:seeAlso rdf:resource="#JavaRmiLibrary"/>
		<rdfs:comment xml:lang="en">JavaLibrary implementing the java.rmi.dgc package for j2se-1_5</rdfs:comment>
	</owl:Class>
	<owl:Class rdf:about="#JavaRmiRegistryLibrary">
		<owl:equivalentClass rdf:resource="&j2se-1_4;JavaRmiRegistryLibrary"/>
		<rdfs:subClassOf rdf:resource="&java;JavaLibrary"/>
		<rdfs:seeAlso rdf:resource="#JavaRmiServerLibrary"/>
		<rdfs:seeAlso rdf:resource="#JavaLangLibrary"/>
		<rdfs:seeAlso rdf:resource="#JavaRmiLibrary"/>
		<rdfs:comment xml:lang="en">JavaLibrary implementing the java.rmi.registry package for j2se-1_5</rdfs:comment>
	</owl:Class>
	<owl:Class rdf:about="#JavaSqlLibrary">
		<owl:equivalentClass rdf:resource="&j2se-1_4;JavaSqlLibrary"/>
		<rdfs:subClassOf rdf:resource="&java;JavaLibrary"/>
		<rdfs:seeAlso rdf:resource="#JavaMathLibrary"/>
		<rdfs:seeAlso rdf:resource="#JavaUtilLibrary"/>
		<rdfs:seeAlso rdf:resource="#JavaLangLibrary"/>
		<rdfs:seeAlso rdf:resource="#JavaNetLibrary"/>
		<rdfs:seeAlso rdf:resource="#JavaIoLibrary"/>
		<rdfs:seeAlso rdf:resource="#JavaSecurityLibrary"/>
		<rdfs:comment xml:lang="en">JavaLibrary implementing the java.sql package for j2se-1_5</rdfs:comment>
	</owl:Class>
	<owl:Class rdf:about="#JavaTextLibrary">
		<rdfs:subClassOf rdf:resource="&java;JavaLibrary"/>
		<rdfs:seeAlso rdf:resource="#JavaUtilLibrary"/>
		<rdfs:seeAlso rdf:resource="#JavaLangLibrary"/>
		<rdfs:seeAlso rdf:resource="#JavaIoLibrary"/>
		<rdfs:comment xml:lang="en">JavaLibrary implementing the java.text package for j2se-1_5</rdfs:comment>
	</owl:Class>
	<owl:Class rdf:about="#JavaxAccessibilityLibrary">
		<rdfs:subClassOf rdf:resource="&j2se-1_4;JavaxAccessibilityLibrary"/>
		<rdfs:seeAlso rdf:resource="#JavaxSwingTextLibrary"/>
		<rdfs:seeAlso rdf:resource="#JavaUtilLibrary"/>
		<rdfs:seeAlso rdf:resource="#JavaBeansLibrary"/>
		<rdfs:seeAlso rdf:resource="#JavaLangLibrary"/>
		<rdfs:seeAlso rdf:resource="#JavaIoLibrary"/>
		<rdfs:seeAlso rdf:resource="#JavaAwtLibrary"/>
		<rdfs:seeAlso rdf:resource="#JavaAwtEventLibrary"/>
		<rdfs:seeAlso rdf:resource="#JavaAwtDatatransferLibrary"/>
		<rdfs:comment xml:lang="en">JavaLibrary implementing the javax.accessibility package for j2se-1_5</rdfs:comment>
	</owl:Class>
	<owl:Class rdf:about="#JavaxSecurityAuthLibrary">
		<owl:equivalentClass rdf:resource="&j2se-1_4;JavaxSecurityAuthLibrary"/>
		<rdfs:subClassOf rdf:resource="&java;JavaLibrary"/>
		<rdfs:seeAlso rdf:resource="#JavaUtilLibrary"/>
		<rdfs:seeAlso rdf:resource="#JavaLangLibrary"/>
		<rdfs:seeAlso rdf:resource="#JavaIoLibrary"/>
		<rdfs:seeAlso rdf:resource="#JavaSecurityLibrary"/>
		<rdfs:comment xml:lang="en">JavaLibrary implementing the javax.security.auth package for j2se-1_5</rdfs:comment>
	</owl:Class>
	<owl:Class rdf:about="#JavaxSecurityAuthCallbackLibrary">
		<owl:equivalentClass rdf:resource="&j2se-1_4;JavaxSecurityAuthCallbackLibrary"/>
		<rdfs:subClassOf rdf:resource="&java;JavaLibrary"/>
		<rdfs:seeAlso rdf:resource="#JavaUtilLibrary"/>
		<rdfs:seeAlso rdf:resource="#JavaIoLibrary"/>
		<rdfs:seeAlso rdf:resource="#JavaLangLibrary"/>
		<rdfs:comment xml:lang="en">JavaLibrary implementing the javax.security.auth.callback package for j2se-1_5</rdfs:comment>
	</owl:Class>
	<owl:Class rdf:about="#JavaxSecurityAuthKerberosLibrary">
		<owl:equivalentClass rdf:resource="&j2se-1_4;JavaxSecurityAuthKerberosLibrary"/>
		<rdfs:subClassOf rdf:resource="&java;JavaLibrary"/>
		<rdfs:seeAlso rdf:resource="#JavaUtilLibrary"/>
		<rdfs:seeAlso rdf:resource="#JavaIoLibrary"/>
		<rdfs:seeAlso rdf:resource="#JavaxSecurityAuthLibrary"/>
		<rdfs:seeAlso rdf:resource="#JavaLangLibrary"/>
		<rdfs:seeAlso rdf:resource="#JavaSecurityLibrary"/>
		<rdfs:seeAlso rdf:resource="#JavaxCryptoLibrary"/>
		<rdfs:comment xml:lang="en">JavaLibrary implementing the javax.security.auth.kerberos package for j2se-1_5</rdfs:comment>
	</owl:Class>
	<owl:Class rdf:about="#JavaxSecurityAuthLoginLibrary">
		<rdfs:subClassOf rdf:resource="&j2se-1_4;JavaxSecurityAuthLoginLibrary"/>
		<rdfs:seeAlso rdf:resource="#JavaxSecurityAuthCallbackLibrary"/>
		<rdfs:seeAlso rdf:resource="#JavaxSecurityAuthLibrary"/>
		<rdfs:seeAlso rdf:resource="#JavaUtilLibrary"/>
		<rdfs:seeAlso rdf:resource="#JavaLangLibrary"/>
		<rdfs:seeAlso rdf:resource="#JavaSecurityLibrary"/>
		<rdfs:comment xml:lang="en">JavaLibrary implementing the javax.security.auth.login package for j2se-1_5</rdfs:comment>
	</owl:Class>
	<owl:Class rdf:about="#JavaxSecurityAuthSpiLibrary">
		<owl:equivalentClass rdf:resource="&j2se-1_4;JavaxSecurityAuthSpiLibrary"/>
		<rdfs:subClassOf rdf:resource="&java;JavaLibrary"/>
		<rdfs:seeAlso rdf:resource="#JavaxSecurityAuthCallbackLibrary"/>
		<rdfs:seeAlso rdf:resource="#JavaUtilLibrary"/>
		<rdfs:seeAlso rdf:resource="#JavaxSecurityAuthLibrary"/>
		<rdfs:comment xml:lang="en">JavaLibrary implementing the javax.security.auth.spi package for j2se-1_5</rdfs:comment>
	</owl:Class>
	<owl:Class rdf:about="#JavaxSecurityAuthX500Library">
		<owl:equivalentClass rdf:resource="&j2se-1_4;JavaxSecurityAuthX500Library"/>
		<rdfs:subClassOf rdf:resource="&java;JavaLibrary"/>
		<rdfs:seeAlso rdf:resource="#JavaSecurityCertLibrary"/>
		<rdfs:seeAlso rdf:resource="#JavaxSecurityAuthLibrary"/>
		<rdfs:seeAlso rdf:resource="#JavaIoLibrary"/>
		<rdfs:seeAlso rdf:resource="#JavaLangLibrary"/>
		<rdfs:seeAlso rdf:resource="#JavaSecurityLibrary"/>
		<rdfs:comment xml:lang="en">JavaLibrary implementing the javax.security.auth.x500 package for j2se-1_5</rdfs:comment>
	</owl:Class>
	<owl:Class rdf:about="#JavaxSecuritySaslLibrary">
		<rdfs:subClassOf rdf:resource="&java;JavaLibrary"/>
		<rdfs:seeAlso rdf:resource="#JavaxSecurityAuthCallbackLibrary"/>
		<rdfs:seeAlso rdf:resource="#JavaIoLibrary"/>
		<rdfs:seeAlso rdf:resource="#JavaUtilLibrary"/>
		<rdfs:seeAlso rdf:resource="#JavaLangLibrary"/>
		<rdfs:comment xml:lang="en">JavaLibrary implementing the javax.security.sasl package for j2se-1_5</rdfs:comment>
	</owl:Class>
	<owl:Class rdf:about="#JavaxActivityLibrary">
		<rdfs:subClassOf rdf:resource="&java;JavaLibrary"/>
		<rdfs:seeAlso rdf:resource="#JavaLangLibrary"/>
		<rdfs:seeAlso rdf:resource="#JavaRmiLibrary"/>
		<rdfs:comment xml:lang="en">JavaLibrary implementing the javax.activity package for j2se-1_5</rdfs:comment>
	</owl:Class>
	<owl:Class rdf:about="#JavaxImageioLibrary">
		<owl:equivalentClass rdf:resource="&j2se-1_4;JavaxImageioLibrary"/>
		<rdfs:subClassOf rdf:resource="&java;JavaLibrary"/>
		<rdfs:seeAlso rdf:resource="#JavaxImageioMetadataLibrary"/>
		<rdfs:seeAlso rdf:resource="#JavaNetLibrary"/>
		<rdfs:seeAlso rdf:resource="#JavaIoLibrary"/>
		<rdfs:seeAlso rdf:resource="#JavaAwtLibrary"/>
		<rdfs:seeAlso rdf:resource="#JavaAwtImageLibrary"/>
		<rdfs:seeAlso rdf:resource="#JavaAwtColorLibrary"/>
		<rdfs:seeAlso rdf:resource="#JavaUtilLibrary"/>
		<rdfs:seeAlso rdf:resource="#JavaLangLibrary"/>
		<rdfs:seeAlso rdf:resource="#JavaxImageioSpiLibrary"/>
		<rdfs:seeAlso rdf:resource="#JavaxImageioEventLibrary"/>
		<rdfs:seeAlso rdf:resource="#JavaxImageioStreamLibrary"/>
		<rdfs:comment xml:lang="en">JavaLibrary implementing the javax.imageio package for j2se-1_5</rdfs:comment>
	</owl:Class>
	<owl:Class rdf:about="#JavaxImageioEventLibrary">
		<owl:equivalentClass rdf:resource="&j2se-1_4;JavaxImageioEventLibrary"/>
		<rdfs:subClassOf rdf:resource="&java;JavaLibrary"/>
		<rdfs:seeAlso rdf:resource="#JavaUtilLibrary"/>
		<rdfs:seeAlso rdf:resource="#JavaLangLibrary"/>
		<rdfs:seeAlso rdf:resource="#JavaxImageioLibrary"/>
		<rdfs:seeAlso rdf:resource="#JavaAwtImageLibrary"/>
		<rdfs:comment xml:lang="en">JavaLibrary implementing the javax.imageio.event package for j2se-1_5</rdfs:comment>
	</owl:Class>
	<owl:Class rdf:about="#JavaxImageioMetadataLibrary">
		<rdfs:subClassOf rdf:resource="&j2se-1_4;JavaxImageioMetadataLibrary"/>
		<rdfs:seeAlso rdf:resource="#JavaUtilLibrary"/>
		<rdfs:seeAlso rdf:resource="#JavaLangLibrary"/>
		<rdfs:seeAlso rdf:resource="#OrgW3cDomLibrary"/>
		<rdfs:seeAlso rdf:resource="#JavaxImageioLibrary"/>
		<rdfs:comment xml:lang="en">JavaLibrary implementing the javax.imageio.metadata package for j2se-1_5</rdfs:comment>
	</owl:Class>
	<owl:Class rdf:about="#JavaxImageioPluginsBmpLibrary">
		<rdfs:subClassOf rdf:resource="&java;JavaLibrary"/>
		<rdfs:seeAlso rdf:resource="#JavaUtilLibrary"/>
		<rdfs:seeAlso rdf:resource="#JavaxImageioLibrary"/>
		<rdfs:comment xml:lang="en">JavaLibrary implementing the javax.imageio.plugins.bmp package for j2se-1_5</rdfs:comment>
	</owl:Class>
	<owl:Class rdf:about="#JavaxImageioPluginsJpegLibrary">
		<owl:equivalentClass rdf:resource="&j2se-1_4;JavaxImageioPluginsJpegLibrary"/>
		<rdfs:subClassOf rdf:resource="&java;JavaLibrary"/>
		<rdfs:seeAlso rdf:resource="#JavaUtilLibrary"/>
		<rdfs:seeAlso rdf:resource="#JavaLangLibrary"/>
		<rdfs:seeAlso rdf:resource="#JavaxImageioLibrary"/>
		<rdfs:comment xml:lang="en">JavaLibrary implementing the javax.imageio.plugins.jpeg package for j2se-1_5</rdfs:comment>
	</owl:Class>
	<owl:Class rdf:about="#JavaxImageioSpiLibrary">
		<owl:equivalentClass rdf:resource="&j2se-1_4;JavaxImageioSpiLibrary"/>
		<rdfs:subClassOf rdf:resource="&java;JavaLibrary"/>
		<rdfs:seeAlso rdf:resource="#JavaUtilLibrary"/>
		<rdfs:seeAlso rdf:resource="#JavaLangLibrary"/>
		<rdfs:seeAlso rdf:resource="#JavaxImageioMetadataLibrary"/>
		<rdfs:seeAlso rdf:resource="#JavaIoLibrary"/>
		<rdfs:seeAlso rdf:resource="#JavaxImageioStreamLibrary"/>
		<rdfs:seeAlso rdf:resource="#JavaxImageioLibrary"/>
		<rdfs:seeAlso rdf:resource="#JavaAwtImageLibrary"/>
		<rdfs:comment xml:lang="en">JavaLibrary implementing the javax.imageio.spi package for j2se-1_5</rdfs:comment>
	</owl:Class>
	<owl:Class rdf:about="#JavaxImageioStreamLibrary">
		<owl:equivalentClass rdf:resource="&j2se-1_4;JavaxImageioStreamLibrary"/>
		<rdfs:subClassOf rdf:resource="&java;JavaLibrary"/>
		<rdfs:seeAlso rdf:resource="#JavaIoLibrary"/>
		<rdfs:seeAlso rdf:resource="#JavaLangLibrary"/>
		<rdfs:seeAlso rdf:resource="#JavaNioLibrary"/>
		<rdfs:comment xml:lang="en">JavaLibrary implementing the javax.imageio.stream package for j2se-1_5</rdfs:comment>
	</owl:Class>
	<owl:Class rdf:about="#JavaxManagementLibrary">
		<rdfs:subClassOf rdf:resource="&java;JavaLibrary"/>
		<rdfs:seeAlso rdf:resource="#JavaxManagementLoadingLibrary"/>
		<rdfs:seeAlso rdf:resource="#JavaIoLibrary"/>
		<rdfs:seeAlso rdf:resource="#JavaSecurityLibrary"/>
		<rdfs:seeAlso rdf:resource="#JavaUtilLibrary"/>
		<rdfs:seeAlso rdf:resource="#JavaLangLibrary"/>
		<rdfs:seeAlso rdf:resource="#JavaLangReflectLibrary"/>
		<rdfs:comment xml:lang="en">JavaLibrary implementing the javax.management package for j2se-1_5</rdfs:comment>
	</owl:Class>
	<owl:Class rdf:about="#JavaxManagementLoadingLibrary">
		<rdfs:subClassOf rdf:resource="&java;JavaLibrary"/>
		<rdfs:seeAlso rdf:resource="#JavaUtilLibrary"/>
		<rdfs:seeAlso rdf:resource="#JavaLangLibrary"/>
		<rdfs:seeAlso rdf:resource="#JavaNetLibrary"/>
		<rdfs:seeAlso rdf:resource="#JavaIoLibrary"/>
		<rdfs:seeAlso rdf:resource="#JavaxManagementLibrary"/>
		<rdfs:comment xml:lang="en">JavaLibrary implementing the javax.management.loading package for j2se-1_5</rdfs:comment>
	</owl:Class>
	<owl:Class rdf:about="#JavaxManagementModelmbeanLibrary">
		<rdfs:subClassOf rdf:resource="&java;JavaLibrary"/>
		<rdfs:seeAlso rdf:resource="#JavaxManagementLoadingLibrary"/>
		<rdfs:seeAlso rdf:resource="#JavaIoLibrary"/>
		<rdfs:seeAlso rdf:resource="#JavaxManagementLibrary"/>
		<rdfs:seeAlso rdf:resource="#JavaLangLibrary"/>
		<rdfs:seeAlso rdf:resource="#JavaLangReflectLibrary"/>
		<rdfs:comment xml:lang="en">JavaLibrary implementing the javax.management.modelmbean package for j2se-1_5</rdfs:comment>
	</owl:Class>
	<owl:Class rdf:about="#JavaxManagementMonitorLibrary">
		<rdfs:subClassOf rdf:resource="&java;JavaLibrary"/>
		<rdfs:seeAlso rdf:resource="#JavaLangLibrary"/>
		<rdfs:seeAlso rdf:resource="#JavaxManagementLibrary"/>
		<rdfs:comment xml:lang="en">JavaLibrary implementing the javax.management.monitor package for j2se-1_5</rdfs:comment>
	</owl:Class>
	<owl:Class rdf:about="#JavaxManagementOpenmbeanLibrary">
		<rdfs:subClassOf rdf:resource="&java;JavaLibrary"/>
		<rdfs:seeAlso rdf:resource="#JavaUtilLibrary"/>
		<rdfs:seeAlso rdf:resource="#JavaLangLibrary"/>
		<rdfs:seeAlso rdf:resource="#JavaIoLibrary"/>
		<rdfs:seeAlso rdf:resource="#JavaxManagementLibrary"/>
		<rdfs:comment xml:lang="en">JavaLibrary implementing the javax.management.openmbean package for j2se-1_5</rdfs:comment>
	</owl:Class>
	<owl:Class rdf:about="#JavaxManagementRelationLibrary">
		<rdfs:subClassOf rdf:resource="&java;JavaLibrary"/>
		<rdfs:seeAlso rdf:resource="#JavaUtilLibrary"/>
		<rdfs:seeAlso rdf:resource="#JavaLangLibrary"/>
		<rdfs:seeAlso rdf:resource="#JavaIoLibrary"/>
		<rdfs:seeAlso rdf:resource="#JavaxManagementLibrary"/>
		<rdfs:comment xml:lang="en">JavaLibrary implementing the javax.management.relation package for j2se-1_5</rdfs:comment>
	</owl:Class>
	<owl:Class rdf:about="#JavaxManagementRemoteLibrary">
		<rdfs:subClassOf rdf:resource="&java;JavaLibrary"/>
		<rdfs:seeAlso rdf:resource="#JavaxSecurityAuthLibrary"/>
		<rdfs:seeAlso rdf:resource="#JavaUtilLibrary"/>
		<rdfs:seeAlso rdf:resource="#JavaLangLibrary"/>
		<rdfs:seeAlso rdf:resource="#JavaIoLibrary"/>
		<rdfs:seeAlso rdf:resource="#JavaSecurityLibrary"/>
		<rdfs:seeAlso rdf:resource="#JavaxManagementLibrary"/>
		<rdfs:comment xml:lang="en">JavaLibrary implementing the javax.management.remote package for j2se-1_5</rdfs:comment>
	</owl:Class>
	<owl:Class rdf:about="#JavaxManagementRemoteRmiLibrary">
		<rdfs:subClassOf rdf:resource="&java;JavaLibrary"/>
		<rdfs:seeAlso rdf:resource="#JavaxManagementRemoteLibrary"/>
		<rdfs:seeAlso rdf:resource="#JavaRmiLibrary"/>
		<rdfs:seeAlso rdf:resource="#JavaIoLibrary"/>
		<rdfs:seeAlso rdf:resource="#JavaRmiServerLibrary"/>
		<rdfs:seeAlso rdf:resource="#JavaxManagementLibrary"/>
		<rdfs:seeAlso rdf:resource="#JavaxSecurityAuthLibrary"/>
		<rdfs:seeAlso rdf:resource="#JavaUtilLibrary"/>
		<rdfs:seeAlso rdf:resource="#JavaLangLibrary"/>
		<rdfs:comment xml:lang="en">JavaLibrary implementing the javax.management.remote.rmi package for j2se-1_5</rdfs:comment>
	</owl:Class>
	<owl:Class rdf:about="#JavaxManagementTimerLibrary">
		<rdfs:subClassOf rdf:resource="&java;JavaLibrary"/>
		<rdfs:seeAlso rdf:resource="#JavaUtilLibrary"/>
		<rdfs:seeAlso rdf:resource="#JavaLangLibrary"/>
		<rdfs:seeAlso rdf:resource="#JavaxManagementLibrary"/>
		<rdfs:comment xml:lang="en">JavaLibrary implementing the javax.management.timer package for j2se-1_5</rdfs:comment>
	</owl:Class>
	<owl:Class rdf:about="#JavaxNamingLibrary">
		<rdfs:subClassOf rdf:resource="&j2se-1_4;JavaxNamingLibrary"/>
		<rdfs:seeAlso rdf:resource="#JavaIoLibrary"/>
		<rdfs:seeAlso rdf:resource="#JavaUtilLibrary"/>
		<rdfs:seeAlso rdf:resource="#JavaLangLibrary"/>
		<rdfs:comment xml:lang="en">JavaLibrary implementing the javax.naming package for j2se-1_5</rdfs:comment>
	</owl:Class>
	<owl:Class rdf:about="#JavaxNamingDirectoryLibrary">
		<rdfs:subClassOf rdf:resource="&j2se-1_4;JavaxNamingDirectoryLibrary"/>
		<rdfs:seeAlso rdf:resource="#JavaUtilLibrary"/>
		<rdfs:seeAlso rdf:resource="#JavaxNamingLibrary"/>
		<rdfs:seeAlso rdf:resource="#JavaLangLibrary"/>
		<rdfs:seeAlso rdf:resource="#JavaIoLibrary"/>
		<rdfs:comment xml:lang="en">JavaLibrary implementing the javax.naming.directory package for j2se-1_5</rdfs:comment>
	</owl:Class>
	<owl:Class rdf:about="#JavaxNamingEventLibrary">
		<owl:equivalentClass rdf:resource="&j2se-1_4;JavaxNamingEventLibrary"/>
		<rdfs:subClassOf rdf:resource="&java;JavaLibrary"/>
		<rdfs:seeAlso rdf:resource="#JavaxNamingDirectoryLibrary"/>
		<rdfs:seeAlso rdf:resource="#JavaUtilLibrary"/>
		<rdfs:seeAlso rdf:resource="#JavaxNamingLibrary"/>
		<rdfs:seeAlso rdf:resource="#JavaLangLibrary"/>
		<rdfs:comment xml:lang="en">JavaLibrary implementing the javax.naming.event package for j2se-1_5</rdfs:comment>
	</owl:Class>
	<owl:Class rdf:about="#JavaxNamingLdapLibrary">
		<rdfs:subClassOf rdf:resource="&j2se-1_4;JavaxNamingLdapLibrary"/>
		<rdfs:seeAlso rdf:resource="#JavaUtilLibrary"/>
		<rdfs:seeAlso rdf:resource="#JavaxNamingLibrary"/>
		<rdfs:seeAlso rdf:resource="#JavaLangLibrary"/>
		<rdfs:seeAlso rdf:resource="#JavaxNamingEventLibrary"/>
		<rdfs:seeAlso rdf:resource="#JavaxNamingDirectoryLibrary"/>
		<rdfs:seeAlso rdf:resource="#JavaIoLibrary"/>
		<rdfs:comment xml:lang="en">JavaLibrary implementing the javax.naming.ldap package for j2se-1_5</rdfs:comment>
	</owl:Class>
	<owl:Class rdf:about="#JavaxNamingSpiLibrary">
		<owl:equivalentClass rdf:resource="&j2se-1_4;JavaxNamingSpiLibrary"/>
		<rdfs:subClassOf rdf:resource="&java;JavaLibrary"/>
		<rdfs:seeAlso rdf:resource="#JavaxNamingDirectoryLibrary"/>
		<rdfs:seeAlso rdf:resource="#JavaUtilLibrary"/>
		<rdfs:seeAlso rdf:resource="#JavaIoLibrary"/>
		<rdfs:seeAlso rdf:resource="#JavaxNamingLibrary"/>
		<rdfs:seeAlso rdf:resource="#JavaLangLibrary"/>
		<rdfs:comment xml:lang="en">JavaLibrary implementing the javax.naming.spi package for j2se-1_5</rdfs:comment>
	</owl:Class>
	<owl:Class rdf:about="#JavaxPrintLibrary">
		<owl:equivalentClass rdf:resource="&j2se-1_4;JavaxPrintLibrary"/>
		<rdfs:subClassOf rdf:resource="&java;JavaLibrary"/>
		<rdfs:seeAlso rdf:resource="#JavaLangLibrary"/>
		<rdfs:seeAlso rdf:resource="#JavaxPrintAttributeLibrary"/>
		<rdfs:seeAlso rdf:resource="#JavaNetLibrary"/>
		<rdfs:seeAlso rdf:resource="#JavaIoLibrary"/>
		<rdfs:seeAlso rdf:resource="#JavaAwtLibrary"/>
		<rdfs:seeAlso rdf:resource="#JavaxPrintEventLibrary"/>
		<rdfs:comment xml:lang="en">JavaLibrary implementing the javax.print package for j2se-1_5</rdfs:comment>
	</owl:Class>
	<owl:Class rdf:about="#JavaxPrintAttributeLibrary">
		<owl:equivalentClass rdf:resource="&j2se-1_4;JavaxPrintAttributeLibrary"/>
		<rdfs:subClassOf rdf:resource="&java;JavaLibrary"/>
		<rdfs:seeAlso rdf:resource="#JavaUtilLibrary"/>
		<rdfs:seeAlso rdf:resource="#JavaIoLibrary"/>
		<rdfs:seeAlso rdf:resource="#JavaLangLibrary"/>
		<rdfs:seeAlso rdf:resource="#JavaNetLibrary"/>
		<rdfs:comment xml:lang="en">JavaLibrary implementing the javax.print.attribute package for j2se-1_5</rdfs:comment>
	</owl:Class>
	<owl:Class rdf:about="#JavaxPrintAttributeStandardLibrary">
		<rdfs:subClassOf rdf:resource="&j2se-1_4;JavaxPrintAttributeStandardLibrary"/>
		<rdfs:seeAlso rdf:resource="#JavaxPrintAttributeLibrary"/>
		<rdfs:seeAlso rdf:resource="#JavaNetLibrary"/>
		<rdfs:seeAlso rdf:resource="#JavaUtilLibrary"/>
		<rdfs:seeAlso rdf:resource="#JavaLangLibrary"/>
		<rdfs:comment xml:lang="en">JavaLibrary implementing the javax.print.attribute.standard package for j2se-1_5</rdfs:comment>
	</owl:Class>
	<owl:Class rdf:about="#JavaxPrintEventLibrary">
		<owl:equivalentClass rdf:resource="&j2se-1_4;JavaxPrintEventLibrary"/>
		<rdfs:subClassOf rdf:resource="&java;JavaLibrary"/>
		<rdfs:seeAlso rdf:resource="#JavaUtilLibrary"/>
		<rdfs:seeAlso rdf:resource="#JavaLangLibrary"/>
		<rdfs:seeAlso rdf:resource="#JavaxPrintAttributeLibrary"/>
		<rdfs:seeAlso rdf:resource="#JavaxPrintLibrary"/>
		<rdfs:comment xml:lang="en">JavaLibrary implementing the javax.print.event package for j2se-1_5</rdfs:comment>
	</owl:Class>
	<owl:Class rdf:about="#JavaxRmiLibrary">
		<owl:equivalentClass rdf:resource="&j2se-1_4;JavaxRmiLibrary"/>
		<rdfs:subClassOf rdf:resource="&java;JavaLibrary"/>
		<rdfs:seeAlso rdf:resource="#JavaLangLibrary"/>
		<rdfs:seeAlso rdf:resource="#JavaRmiLibrary"/>
		<rdfs:comment xml:lang="en">JavaLibrary implementing the javax.rmi package for j2se-1_5</rdfs:comment>
	</owl:Class>
	<owl:Class rdf:about="#JavaxRmiCORBALibrary">
		<rdfs:subClassOf rdf:resource="&j2se-1_4;JavaxRmiCORBALibrary"/>
		<rdfs:seeAlso rdf:resource="#OrgOmgSendingContextLibrary"/>
		<rdfs:seeAlso rdf:resource="#JavaLangLibrary"/>
		<rdfs:seeAlso rdf:resource="#OrgOmgCORBAPortableLibrary"/>
		<rdfs:seeAlso rdf:resource="#OrgOmgCORBA_2_3PortableLibrary"/>
		<rdfs:seeAlso rdf:resource="#JavaRmiLibrary"/>
		<rdfs:seeAlso rdf:resource="#JavaIoLibrary"/>
		<rdfs:seeAlso rdf:resource="#OrgOmgCORBALibrary"/>
		<rdfs:comment xml:lang="en">JavaLibrary implementing the javax.rmi.CORBA package for j2se-1_5</rdfs:comment>
	</owl:Class>
	<owl:Class rdf:about="#JavaxRmiSslLibrary">
		<rdfs:subClassOf rdf:resource="&java;JavaLibrary"/>
		<rdfs:seeAlso rdf:resource="#JavaIoLibrary"/>
		<rdfs:seeAlso rdf:resource="#JavaRmiServerLibrary"/>
		<rdfs:seeAlso rdf:resource="#JavaLangLibrary"/>
		<rdfs:seeAlso rdf:resource="#JavaNetLibrary"/>
		<rdfs:comment xml:lang="en">JavaLibrary implementing the javax.rmi.ssl package for j2se-1_5</rdfs:comment>
	</owl:Class>
	<owl:Class rdf:about="#JavaxCryptoLibrary">
		<owl:equivalentClass rdf:resource="&j2se-1_4;JavaxCryptoLibrary"/>
		<rdfs:subClassOf rdf:resource="&java;JavaLibrary"/>
		<rdfs:comment xml:lang="en">JavaLibrary implementing the javax.crypto package for j2se-1_5</rdfs:comment>
	</owl:Class>
	<owl:Class rdf:about="#JavaxSoundMidiLibrary">
		<rdfs:subClassOf rdf:resource="&java;JavaLibrary"/>
		<rdfs:seeAlso rdf:resource="#JavaUtilLibrary"/>
		<rdfs:seeAlso rdf:resource="#JavaLangLibrary"/>
		<rdfs:seeAlso rdf:resource="#JavaNetLibrary"/>
		<rdfs:seeAlso rdf:resource="#JavaIoLibrary"/>
		<rdfs:comment xml:lang="en">JavaLibrary implementing the javax.sound.midi package for j2se-1_5</rdfs:comment>
	</owl:Class>
	<owl:Class rdf:about="#JavaxSoundMidiSpiLibrary">
		<owl:equivalentClass rdf:resource="&j2se-1_4;JavaxSoundMidiSpiLibrary"/>
		<rdfs:subClassOf rdf:resource="&java;JavaLibrary"/>
		<rdfs:seeAlso rdf:resource="#JavaIoLibrary"/>
		<rdfs:seeAlso rdf:resource="#JavaLangLibrary"/>
		<rdfs:seeAlso rdf:resource="#JavaNetLibrary"/>
		<rdfs:seeAlso rdf:resource="#JavaxSoundMidiLibrary"/>
		<rdfs:comment xml:lang="en">JavaLibrary implementing the javax.sound.midi.spi package for j2se-1_5</rdfs:comment>
	</owl:Class>
	<owl:Class rdf:about="#JavaxSoundSampledLibrary">
		<rdfs:subClassOf rdf:resource="&j2se-1_4;JavaxSoundSampledLibrary"/>
		<rdfs:seeAlso rdf:resource="#JavaUtilLibrary"/>
		<rdfs:seeAlso rdf:resource="#JavaLangLibrary"/>
		<rdfs:seeAlso rdf:resource="#JavaNetLibrary"/>
		<rdfs:seeAlso rdf:resource="#JavaIoLibrary"/>
		<rdfs:seeAlso rdf:resource="#JavaSecurityLibrary"/>
		<rdfs:comment xml:lang="en">JavaLibrary implementing the javax.sound.sampled package for j2se-1_5</rdfs:comment>
	</owl:Class>
	<owl:Class rdf:about="#JavaxSoundSampledSpiLibrary">
		<owl:equivalentClass rdf:resource="&j2se-1_4;JavaxSoundSampledSpiLibrary"/>
		<rdfs:subClassOf rdf:resource="&java;JavaLibrary"/>
		<rdfs:seeAlso rdf:resource="#JavaLangLibrary"/>
		<rdfs:seeAlso rdf:resource="#JavaNetLibrary"/>
		<rdfs:seeAlso rdf:resource="#JavaIoLibrary"/>
		<rdfs:seeAlso rdf:resource="#JavaxSoundSampledLibrary"/>
		<rdfs:comment xml:lang="en">JavaLibrary implementing the javax.sound.sampled.spi package for j2se-1_5</rdfs:comment>
	</owl:Class>
	<owl:Class rdf:about="#JavaxSqlLibrary">
		<owl:equivalentClass rdf:resource="&j2se-1_4;JavaxSqlLibrary"/>
		<rdfs:subClassOf rdf:resource="&java;JavaLibrary"/>
		<rdfs:seeAlso rdf:resource="#JavaMathLibrary"/>
		<rdfs:seeAlso rdf:resource="#JavaSqlLibrary"/>
		<rdfs:seeAlso rdf:resource="#JavaUtilLibrary"/>
		<rdfs:seeAlso rdf:resource="#JavaLangLibrary"/>
		<rdfs:seeAlso rdf:resource="#JavaIoLibrary"/>
		<rdfs:seeAlso rdf:resource="#JavaxTransactionXaLibrary"/>
		<rdfs:comment xml:lang="en">JavaLibrary implementing the javax.sql package for j2se-1_5</rdfs:comment>
	</owl:Class>
	<owl:Class rdf:about="#JavaxSqlRowsetLibrary">
		<rdfs:subClassOf rdf:resource="&java;JavaLibrary"/>
		<rdfs:seeAlso rdf:resource="#JavaMathLibrary"/>
		<rdfs:seeAlso rdf:resource="#JavaSqlLibrary"/>
		<rdfs:seeAlso rdf:resource="#JavaxSqlRowsetSpiLibrary"/>
		<rdfs:seeAlso rdf:resource="#JavaIoLibrary"/>
		<rdfs:seeAlso rdf:resource="#JavaUtilLibrary"/>
		<rdfs:seeAlso rdf:resource="#JavaLangLibrary"/>
		<rdfs:seeAlso rdf:resource="#JavaxSqlLibrary"/>
		<rdfs:comment xml:lang="en">JavaLibrary implementing the javax.sql.rowset package for j2se-1_5</rdfs:comment>
	</owl:Class>
	<owl:Class rdf:about="#JavaxSqlRowsetSerialLibrary">
		<rdfs:subClassOf rdf:resource="&java;JavaLibrary"/>
		<rdfs:seeAlso rdf:resource="#JavaMathLibrary"/>
		<rdfs:seeAlso rdf:resource="#JavaSqlLibrary"/>
		<rdfs:seeAlso rdf:resource="#JavaNetLibrary"/>
		<rdfs:seeAlso rdf:resource="#JavaIoLibrary"/>
		<rdfs:seeAlso rdf:resource="#JavaUtilLibrary"/>
		<rdfs:seeAlso rdf:resource="#JavaLangLibrary"/>
		<rdfs:comment xml:lang="en">JavaLibrary implementing the javax.sql.rowset.serial package for j2se-1_5</rdfs:comment>
	</owl:Class>
	<owl:Class rdf:about="#JavaxSqlRowsetSpiLibrary">
		<rdfs:subClassOf rdf:resource="&java;JavaLibrary"/>
		<rdfs:seeAlso rdf:resource="#JavaSqlLibrary"/>
		<rdfs:seeAlso rdf:resource="#JavaUtilLibrary"/>
		<rdfs:seeAlso rdf:resource="#JavaxNamingLibrary"/>
		<rdfs:seeAlso rdf:resource="#JavaLangLibrary"/>
		<rdfs:seeAlso rdf:resource="#JavaxSqlLibrary"/>
		<rdfs:seeAlso rdf:resource="#JavaxSqlRowsetLibrary"/>
		<rdfs:seeAlso rdf:resource="#JavaIoLibrary"/>
		<rdfs:seeAlso rdf:resource="#JavaUtilLoggingLibrary"/>
		<rdfs:comment xml:lang="en">JavaLibrary implementing the javax.sql.rowset.spi package for j2se-1_5</rdfs:comment>
	</owl:Class>
	<owl:Class rdf:about="#JavaxSwingLibrary">
		<rdfs:subClassOf rdf:resource="&j2se-1_4;JavaxSwingLibrary"/>
		<rdfs:seeAlso rdf:resource="#JavaxAccessibilityLibrary"/>
		<rdfs:seeAlso rdf:resource="#JavaAppletLibrary"/>
		<rdfs:seeAlso rdf:resource="#JavaxSwingTableLibrary"/>
		<rdfs:seeAlso rdf:resource="#JavaIoLibrary"/>
		<rdfs:seeAlso rdf:resource="#JavaAwtDatatransferLibrary"/>
		<rdfs:seeAlso rdf:resource="#JavaxSwingBorderLibrary"/>
		<rdfs:seeAlso rdf:resource="#JavaAwtLibrary"/>
		<rdfs:seeAlso rdf:resource="#JavaAwtImageLibrary"/>
		<rdfs:seeAlso rdf:resource="#JavaxSwingPlafLibrary"/>
		<rdfs:seeAlso rdf:resource="#JavaUtilLibrary"/>
		<rdfs:seeAlso rdf:resource="#JavaTextLibrary"/>
		<rdfs:seeAlso rdf:resource="#JavaxPrintAttributeLibrary"/>
		<rdfs:seeAlso rdf:resource="#JavaxSwingEventLibrary"/>
		<rdfs:seeAlso rdf:resource="#JavaxSwingFilechooserLibrary"/>
		<rdfs:seeAlso rdf:resource="#JavaLangLibrary"/>
		<rdfs:seeAlso rdf:resource="#JavaxSwingTextLibrary"/>
		<rdfs:seeAlso rdf:resource="#JavaNetLibrary"/>
		<rdfs:seeAlso rdf:resource="#JavaAwtEventLibrary"/>
		<rdfs:seeAlso rdf:resource="#JavaxSwingColorchooserLibrary"/>
		<rdfs:seeAlso rdf:resource="#JavaAwtPrintLibrary"/>
		<rdfs:seeAlso rdf:resource="#JavaBeansLibrary"/>
		<rdfs:seeAlso rdf:resource="#JavaxSwingTreeLibrary"/>
		<rdfs:comment xml:lang="en">JavaLibrary implementing the javax.swing package for j2se-1_5</rdfs:comment>
	</owl:Class>
	<owl:Class rdf:about="#JavaxSwingTextLibrary">
		<rdfs:subClassOf rdf:resource="&j2se-1_4;JavaxSwingTextLibrary"/>
		<rdfs:seeAlso rdf:resource="#JavaxAccessibilityLibrary"/>
		<rdfs:seeAlso rdf:resource="#JavaxSwingPlafBasicLibrary"/>
		<rdfs:seeAlso rdf:resource="#JavaxSwingLibrary"/>
		<rdfs:seeAlso rdf:resource="#JavaAwtEventLibrary"/>
		<rdfs:seeAlso rdf:resource="#JavaUtilLibrary"/>
		<rdfs:seeAlso rdf:resource="#JavaTextLibrary"/>
		<rdfs:seeAlso rdf:resource="#JavaxSwingUndoLibrary"/>
		<rdfs:seeAlso rdf:resource="#JavaxSwingEventLibrary"/>
		<rdfs:seeAlso rdf:resource="#JavaIoLibrary"/>
		<rdfs:seeAlso rdf:resource="#JavaAwtLibrary"/>
		<rdfs:seeAlso rdf:resource="#JavaxSwingPlafLibrary"/>
		<rdfs:seeAlso rdf:resource="#JavaLangLibrary"/>
		<rdfs:seeAlso rdf:resource="#JavaAwtImLibrary"/>
		<rdfs:seeAlso rdf:resource="#JavaxSwingTreeLibrary"/>
		<rdfs:comment xml:lang="en">JavaLibrary implementing the javax.swing.text package for j2se-1_5</rdfs:comment>
	</owl:Class>
	<owl:Class rdf:about="#JavaxSwingTextHtmlLibrary">
		<rdfs:subClassOf rdf:resource="&j2se-1_4;JavaxSwingTextHtmlLibrary"/>
		<rdfs:seeAlso rdf:resource="#JavaxSwingTextLibrary"/>
		<rdfs:seeAlso rdf:resource="#JavaxAccessibilityLibrary"/>
		<rdfs:seeAlso rdf:resource="#JavaNetLibrary"/>
		<rdfs:seeAlso rdf:resource="#JavaxSwingLibrary"/>
		<rdfs:seeAlso rdf:resource="#JavaAwtEventLibrary"/>
		<rdfs:seeAlso rdf:resource="#JavaUtilLibrary"/>
		<rdfs:seeAlso rdf:resource="#JavaxSwingEventLibrary"/>
		<rdfs:seeAlso rdf:resource="#JavaIoLibrary"/>
		<rdfs:seeAlso rdf:resource="#JavaAwtLibrary"/>
		<rdfs:seeAlso rdf:resource="#JavaLangLibrary"/>
		<rdfs:comment xml:lang="en">JavaLibrary implementing the javax.swing.text.html package for j2se-1_5</rdfs:comment>
	</owl:Class>
	<owl:Class rdf:about="#JavaxSwingTextHtmlParserLibrary">
		<owl:equivalentClass rdf:resource="&j2se-1_4;JavaxSwingTextHtmlParserLibrary"/>
		<rdfs:subClassOf rdf:resource="&java;JavaLibrary"/>
		<rdfs:seeAlso rdf:resource="#JavaxSwingTextLibrary"/>
		<rdfs:seeAlso rdf:resource="#JavaUtilLibrary"/>
		<rdfs:seeAlso rdf:resource="#JavaLangLibrary"/>
		<rdfs:seeAlso rdf:resource="#JavaxSwingTextHtmlLibrary"/>
		<rdfs:seeAlso rdf:resource="#JavaIoLibrary"/>
		<rdfs:comment xml:lang="en">JavaLibrary implementing the javax.swing.text.html.parser package for j2se-1_5</rdfs:comment>
	</owl:Class>
	<owl:Class rdf:about="#JavaxSwingTextRtfLibrary">
		<owl:equivalentClass rdf:resource="&j2se-1_4;JavaxSwingTextRtfLibrary"/>
		<rdfs:subClassOf rdf:resource="&java;JavaLibrary"/>
		<rdfs:seeAlso rdf:resource="#JavaxSwingTextLibrary"/>
		<rdfs:seeAlso rdf:resource="#JavaIoLibrary"/>
		<rdfs:seeAlso rdf:resource="#JavaLangLibrary"/>
		<rdfs:comment xml:lang="en">JavaLibrary implementing the javax.swing.text.rtf package for j2se-1_5</rdfs:comment>
	</owl:Class>
	<owl:Class rdf:about="#JavaxSwingEventLibrary">
		<rdfs:subClassOf rdf:resource="&j2se-1_4;JavaxSwingEventLibrary"/>
		<rdfs:seeAlso rdf:resource="#JavaxSwingTextLibrary"/>
		<rdfs:seeAlso rdf:resource="#JavaxSwingUndoLibrary"/>
		<rdfs:seeAlso rdf:resource="#JavaNetLibrary"/>
		<rdfs:seeAlso rdf:resource="#JavaxSwingTableLibrary"/>
		<rdfs:seeAlso rdf:resource="#JavaIoLibrary"/>
		<rdfs:seeAlso rdf:resource="#JavaxSwingLibrary"/>
		<rdfs:seeAlso rdf:resource="#JavaAwtLibrary"/>
		<rdfs:seeAlso rdf:resource="#JavaAwtEventLibrary"/>
		<rdfs:seeAlso rdf:resource="#JavaUtilLibrary"/>
		<rdfs:seeAlso rdf:resource="#JavaBeansLibrary"/>
		<rdfs:seeAlso rdf:resource="#JavaLangLibrary"/>
		<rdfs:seeAlso rdf:resource="#JavaxSwingTreeLibrary"/>
		<rdfs:comment xml:lang="en">JavaLibrary implementing the javax.swing.event package for j2se-1_5</rdfs:comment>
	</owl:Class>
	<owl:Class rdf:about="#JavaxSwingTreeLibrary">
		<rdfs:subClassOf rdf:resource="&j2se-1_4;JavaxSwingTreeLibrary"/>
		<rdfs:seeAlso rdf:resource="#JavaxSwingEventLibrary"/>
		<rdfs:seeAlso rdf:resource="#JavaIoLibrary"/>
		<rdfs:seeAlso rdf:resource="#JavaxSwingLibrary"/>
		<rdfs:seeAlso rdf:resource="#JavaAwtLibrary"/>
		<rdfs:seeAlso rdf:resource="#JavaAwtEventLibrary"/>
		<rdfs:seeAlso rdf:resource="#JavaUtilLibrary"/>
		<rdfs:seeAlso rdf:resource="#JavaBeansLibrary"/>
		<rdfs:seeAlso rdf:resource="#JavaLangLibrary"/>
		<rdfs:seeAlso rdf:resource="#JavaxSwingBorderLibrary"/>
		<rdfs:comment xml:lang="en">JavaLibrary implementing the javax.swing.tree package for j2se-1_5</rdfs:comment>
	</owl:Class>
	<owl:Class rdf:about="#JavaxSwingBorderLibrary">
		<owl:equivalentClass rdf:resource="&j2se-1_4;JavaxSwingBorderLibrary"/>
		<rdfs:subClassOf rdf:resource="&java;JavaLibrary"/>
		<rdfs:seeAlso rdf:resource="#JavaIoLibrary"/>
		<rdfs:seeAlso rdf:resource="#JavaLangLibrary"/>
		<rdfs:seeAlso rdf:resource="#JavaxSwingLibrary"/>
		<rdfs:seeAlso rdf:resource="#JavaAwtLibrary"/>
		<rdfs:comment xml:lang="en">JavaLibrary implementing the javax.swing.border package for j2se-1_5</rdfs:comment>
	</owl:Class>
	<owl:Class rdf:about="#JavaxSwingColorchooserLibrary">
		<rdfs:subClassOf rdf:resource="&j2se-1_4;JavaxSwingColorchooserLibrary"/>
		<rdfs:seeAlso rdf:resource="#JavaLangLibrary"/>
		<rdfs:seeAlso rdf:resource="#JavaxSwingEventLibrary"/>
		<rdfs:seeAlso rdf:resource="#JavaIoLibrary"/>
		<rdfs:seeAlso rdf:resource="#JavaxSwingLibrary"/>
		<rdfs:seeAlso rdf:resource="#JavaAwtLibrary"/>
		<rdfs:comment xml:lang="en">JavaLibrary implementing the javax.swing.colorchooser package for j2se-1_5</rdfs:comment>
	</owl:Class>
	<owl:Class rdf:about="#JavaxSwingFilechooserLibrary">
		<owl:equivalentClass rdf:resource="&j2se-1_4;JavaxSwingFilechooserLibrary"/>
		<rdfs:subClassOf rdf:resource="&java;JavaLibrary"/>
		<rdfs:seeAlso rdf:resource="#JavaIoLibrary"/>
		<rdfs:seeAlso rdf:resource="#JavaLangLibrary"/>
		<rdfs:seeAlso rdf:resource="#JavaxSwingLibrary"/>
		<rdfs:comment xml:lang="en">JavaLibrary implementing the javax.swing.filechooser package for j2se-1_5</rdfs:comment>
	</owl:Class>
	<owl:Class rdf:about="#JavaxSwingPlafLibrary">
		<rdfs:subClassOf rdf:resource="&j2se-1_4;JavaxSwingPlafLibrary"/>
		<rdfs:seeAlso rdf:resource="#JavaxSwingTextLibrary"/>
		<rdfs:seeAlso rdf:resource="#JavaxAccessibilityLibrary"/>
		<rdfs:seeAlso rdf:resource="#JavaxSwingFilechooserLibrary"/>
		<rdfs:seeAlso rdf:resource="#JavaIoLibrary"/>
		<rdfs:seeAlso rdf:resource="#JavaxSwingLibrary"/>
		<rdfs:seeAlso rdf:resource="#JavaAwtLibrary"/>
		<rdfs:seeAlso rdf:resource="#JavaAwtEventLibrary"/>
		<rdfs:seeAlso rdf:resource="#JavaLangLibrary"/>
		<rdfs:seeAlso rdf:resource="#JavaxSwingTreeLibrary"/>
		<rdfs:seeAlso rdf:resource="#JavaxSwingBorderLibrary"/>
		<rdfs:comment xml:lang="en">JavaLibrary implementing the javax.swing.plaf package for j2se-1_5</rdfs:comment>
	</owl:Class>
	<owl:Class rdf:about="#JavaxSwingPlafBasicLibrary">
		<rdfs:subClassOf rdf:resource="&j2se-1_4;JavaxSwingPlafBasicLibrary"/>
		<rdfs:seeAlso rdf:resource="#JavaxAccessibilityLibrary"/>
		<rdfs:seeAlso rdf:resource="#JavaxSwingTableLibrary"/>
		<rdfs:seeAlso rdf:resource="#JavaUtilLibrary"/>
		<rdfs:seeAlso rdf:resource="#JavaxSwingEventLibrary"/>
		<rdfs:seeAlso rdf:resource="#JavaxSwingFilechooserLibrary"/>
		<rdfs:seeAlso rdf:resource="#JavaIoLibrary"/>
		<rdfs:seeAlso rdf:resource="#JavaLangLibrary"/>
		<rdfs:seeAlso rdf:resource="#JavaxSwingTextLibrary"/>
		<rdfs:seeAlso rdf:resource="#JavaxSwingLibrary"/>
		<rdfs:seeAlso rdf:resource="#JavaAwtEventLibrary"/>
		<rdfs:seeAlso rdf:resource="#JavaxSwingBorderLibrary"/>
		<rdfs:seeAlso rdf:resource="#JavaAwtLibrary"/>
		<rdfs:seeAlso rdf:resource="#JavaBeansLibrary"/>
		<rdfs:seeAlso rdf:resource="#JavaxSwingPlafLibrary"/>
		<rdfs:seeAlso rdf:resource="#JavaxSwingTreeLibrary"/>
		<rdfs:comment xml:lang="en">JavaLibrary implementing the javax.swing.plaf.basic package for j2se-1_5</rdfs:comment>
	</owl:Class>
	<owl:Class rdf:about="#JavaxSwingPlafMetalLibrary">
		<rdfs:subClassOf rdf:resource="&j2se-1_4;JavaxSwingPlafMetalLibrary"/>
		<rdfs:seeAlso rdf:resource="#JavaxSwingPlafBasicLibrary"/>
		<rdfs:seeAlso rdf:resource="#JavaxSwingLibrary"/>
		<rdfs:seeAlso rdf:resource="#JavaAwtEventLibrary"/>
		<rdfs:seeAlso rdf:resource="#JavaxSwingBorderLibrary"/>
		<rdfs:seeAlso rdf:resource="#JavaxSwingEventLibrary"/>
		<rdfs:seeAlso rdf:resource="#JavaIoLibrary"/>
		<rdfs:seeAlso rdf:resource="#JavaAwtLibrary"/>
		<rdfs:seeAlso rdf:resource="#JavaBeansLibrary"/>
		<rdfs:seeAlso rdf:resource="#JavaxSwingPlafLibrary"/>
		<rdfs:seeAlso rdf:resource="#JavaLangLibrary"/>
		<rdfs:seeAlso rdf:resource="#JavaxSwingTreeLibrary"/>
		<rdfs:comment xml:lang="en">JavaLibrary implementing the javax.swing.plaf.metal package for j2se-1_5</rdfs:comment>
	</owl:Class>
	<owl:Class rdf:about="#JavaxSwingPlafMultiLibrary">
		<rdfs:subClassOf rdf:resource="&j2se-1_4;JavaxSwingPlafMultiLibrary"/>
		<rdfs:seeAlso rdf:resource="#JavaxSwingTextLibrary"/>
		<rdfs:seeAlso rdf:resource="#JavaxAccessibilityLibrary"/>
		<rdfs:seeAlso rdf:resource="#JavaxSwingLibrary"/>
		<rdfs:seeAlso rdf:resource="#JavaAwtEventLibrary"/>
		<rdfs:seeAlso rdf:resource="#JavaUtilLibrary"/>
		<rdfs:seeAlso rdf:resource="#JavaxSwingFilechooserLibrary"/>
		<rdfs:seeAlso rdf:resource="#JavaIoLibrary"/>
		<rdfs:seeAlso rdf:resource="#JavaAwtLibrary"/>
		<rdfs:seeAlso rdf:resource="#JavaxSwingPlafLibrary"/>
		<rdfs:seeAlso rdf:resource="#JavaLangLibrary"/>
		<rdfs:seeAlso rdf:resource="#JavaxSwingTreeLibrary"/>
		<rdfs:comment xml:lang="en">JavaLibrary implementing the javax.swing.plaf.multi package for j2se-1_5</rdfs:comment>
	</owl:Class>
	<owl:Class rdf:about="#JavaxSwingPlafSynthLibrary">
		<rdfs:subClassOf rdf:resource="&java;JavaLibrary"/>
		<rdfs:seeAlso rdf:resource="#JavaxSwingPlafLibrary"/>
		<rdfs:seeAlso rdf:resource="#JavaLangLibrary"/>
		<rdfs:seeAlso rdf:resource="#JavaIoLibrary"/>
		<rdfs:seeAlso rdf:resource="#JavaxSwingPlafBasicLibrary"/>
		<rdfs:seeAlso rdf:resource="#JavaxSwingLibrary"/>
		<rdfs:seeAlso rdf:resource="#JavaAwtLibrary"/>
		<rdfs:seeAlso rdf:resource="#JavaAwtEventLibrary"/>
		<rdfs:comment xml:lang="en">JavaLibrary implementing the javax.swing.plaf.synth package for j2se-1_5</rdfs:comment>
	</owl:Class>
	<owl:Class rdf:about="#JavaxSwingTableLibrary">
		<rdfs:subClassOf rdf:resource="&j2se-1_4;JavaxSwingTableLibrary"/>
		<rdfs:seeAlso rdf:resource="#JavaxAccessibilityLibrary"/>
		<rdfs:seeAlso rdf:resource="#JavaxSwingEventLibrary"/>
		<rdfs:seeAlso rdf:resource="#JavaIoLibrary"/>
		<rdfs:seeAlso rdf:resource="#JavaxSwingLibrary"/>
		<rdfs:seeAlso rdf:resource="#JavaAwtLibrary"/>
		<rdfs:seeAlso rdf:resource="#JavaAwtEventLibrary"/>
		<rdfs:seeAlso rdf:resource="#JavaUtilLibrary"/>
		<rdfs:seeAlso rdf:resource="#JavaBeansLibrary"/>
		<rdfs:seeAlso rdf:resource="#JavaxSwingPlafLibrary"/>
		<rdfs:seeAlso rdf:resource="#JavaLangLibrary"/>
		<rdfs:seeAlso rdf:resource="#JavaxSwingBorderLibrary"/>
		<rdfs:comment xml:lang="en">JavaLibrary implementing the javax.swing.table package for j2se-1_5</rdfs:comment>
	</owl:Class>
	<owl:Class rdf:about="#JavaxSwingUndoLibrary">
		<owl:equivalentClass rdf:resource="&j2se-1_4;JavaxSwingUndoLibrary"/>
		<rdfs:subClassOf rdf:resource="&java;JavaLibrary"/>
		<rdfs:seeAlso rdf:resource="#JavaIoLibrary"/>
		<rdfs:seeAlso rdf:resource="#JavaUtilLibrary"/>
		<rdfs:seeAlso rdf:resource="#JavaLangLibrary"/>
		<rdfs:seeAlso rdf:resource="#JavaxSwingEventLibrary"/>
		<rdfs:comment xml:lang="en">JavaLibrary implementing the javax.swing.undo package for j2se-1_5</rdfs:comment>
	</owl:Class>
	<owl:Class rdf:about="#JavaxTransactionLibrary">
		<owl:equivalentClass rdf:resource="&j2se-1_4;JavaxTransactionLibrary"/>
		<rdfs:subClassOf rdf:resource="&java;JavaLibrary"/>
		<rdfs:seeAlso rdf:resource="#JavaLangLibrary"/>
		<rdfs:seeAlso rdf:resource="#JavaRmiLibrary"/>
		<rdfs:comment xml:lang="en">JavaLibrary implementing the javax.transaction package for j2se-1_5</rdfs:comment>
	</owl:Class>
	<owl:Class rdf:about="#JavaxTransactionXaLibrary">
		<owl:equivalentClass rdf:resource="&j2se-1_4;JavaxTransactionXaLibrary"/>
		<rdfs:subClassOf rdf:resource="&java;JavaLibrary"/>
		<rdfs:seeAlso rdf:resource="#JavaLangLibrary"/>
		<rdfs:comment xml:lang="en">JavaLibrary implementing the javax.transaction.xa package for j2se-1_5</rdfs:comment>
	</owl:Class>
	<owl:Class rdf:about="#JavaxXmlLibrary">
		<rdfs:subClassOf rdf:resource="&java;JavaLibrary"/>
		<rdfs:seeAlso rdf:resource="#JavaLangLibrary"/>
		<rdfs:comment xml:lang="en">JavaLibrary implementing the javax.xml package for j2se-1_5</rdfs:comment>
	</owl:Class>
	<owl:Class rdf:about="#JavaxXmlDatatypeLibrary">
		<rdfs:subClassOf rdf:resource="&java;JavaLibrary"/>
		<rdfs:seeAlso rdf:resource="#JavaMathLibrary"/>
		<rdfs:seeAlso rdf:resource="#JavaUtilLibrary"/>
		<rdfs:seeAlso rdf:resource="#JavaxXmlNamespaceLibrary"/>
		<rdfs:seeAlso rdf:resource="#JavaLangLibrary"/>
		<rdfs:comment xml:lang="en">JavaLibrary implementing the javax.xml.datatype package for j2se-1_5</rdfs:comment>
	</owl:Class>
	<owl:Class rdf:about="#JavaxXmlNamespaceLibrary">
		<rdfs:subClassOf rdf:resource="&java;JavaLibrary"/>
		<rdfs:seeAlso rdf:resource="#JavaIoLibrary"/>
		<rdfs:seeAlso rdf:resource="#JavaUtilLibrary"/>
		<rdfs:seeAlso rdf:resource="#JavaLangLibrary"/>
		<rdfs:comment xml:lang="en">JavaLibrary implementing the javax.xml.namespace package for j2se-1_5</rdfs:comment>
	</owl:Class>
	<owl:Class rdf:about="#JavaxXmlParsersLibrary">
		<rdfs:subClassOf rdf:resource="&j2se-1_4;JavaxXmlParsersLibrary"/>
		<rdfs:seeAlso rdf:resource="#JavaLangLibrary"/>
		<rdfs:seeAlso rdf:resource="#OrgXmlSaxHelpersLibrary"/>
		<rdfs:seeAlso rdf:resource="#OrgW3cDomLibrary"/>
		<rdfs:seeAlso rdf:resource="#JavaIoLibrary"/>
		<rdfs:seeAlso rdf:resource="#OrgXmlSaxLibrary"/>
		<rdfs:seeAlso rdf:resource="#JavaxXmlValidationLibrary"/>
		<rdfs:comment xml:lang="en">JavaLibrary implementing the javax.xml.parsers package for j2se-1_5</rdfs:comment>
	</owl:Class>
	<owl:Class rdf:about="#JavaxXmlTransformLibrary">
		<rdfs:subClassOf rdf:resource="&j2se-1_4;JavaxXmlTransformLibrary"/>
		<rdfs:seeAlso rdf:resource="#JavaUtilLibrary"/>
		<rdfs:seeAlso rdf:resource="#JavaIoLibrary"/>
		<rdfs:seeAlso rdf:resource="#JavaLangLibrary"/>
		<rdfs:comment xml:lang="en">JavaLibrary implementing the javax.xml.transform package for j2se-1_5</rdfs:comment>
	</owl:Class>
	<owl:Class rdf:about="#JavaxXmlTransformDomLibrary">
		<rdfs:subClassOf rdf:resource="&j2se-1_4;JavaxXmlTransformDomLibrary"/>
		<rdfs:seeAlso rdf:resource="#OrgW3cDomLibrary"/>
		<rdfs:seeAlso rdf:resource="#JavaLangLibrary"/>
		<rdfs:seeAlso rdf:resource="#JavaxXmlTransformLibrary"/>
		<rdfs:comment xml:lang="en">JavaLibrary implementing the javax.xml.transform.dom package for j2se-1_5</rdfs:comment>
	</owl:Class>
	<owl:Class rdf:about="#JavaxXmlTransformSaxLibrary">
		<rdfs:subClassOf rdf:resource="&j2se-1_4;JavaxXmlTransformSaxLibrary"/>
		<rdfs:seeAlso rdf:resource="#JavaLangLibrary"/>
		<rdfs:seeAlso rdf:resource="#OrgXmlSaxExtLibrary"/>
		<rdfs:seeAlso rdf:resource="#OrgXmlSaxLibrary"/>
		<rdfs:seeAlso rdf:resource="#JavaxXmlTransformLibrary"/>
		<rdfs:comment xml:lang="en">JavaLibrary implementing the javax.xml.transform.sax package for j2se-1_5</rdfs:comment>
	</owl:Class>
	<owl:Class rdf:about="#JavaxXmlTransformStreamLibrary">
		<owl:equivalentClass rdf:resource="&j2se-1_4;JavaxXmlTransformStreamLibrary"/>
		<rdfs:subClassOf rdf:resource="&java;JavaLibrary"/>
		<rdfs:seeAlso rdf:resource="#JavaIoLibrary"/>
		<rdfs:seeAlso rdf:resource="#JavaLangLibrary"/>
		<rdfs:seeAlso rdf:resource="#JavaxXmlTransformLibrary"/>
		<rdfs:comment xml:lang="en">JavaLibrary implementing the javax.xml.transform.stream package for j2se-1_5</rdfs:comment>
	</owl:Class>
	<owl:Class rdf:about="#JavaxXmlValidationLibrary">
		<rdfs:subClassOf rdf:resource="&java;JavaLibrary"/>
		<rdfs:seeAlso rdf:resource="#OrgW3cDomLibrary"/>
		<rdfs:seeAlso rdf:resource="#JavaIoLibrary"/>
		<rdfs:seeAlso rdf:resource="#JavaLangLibrary"/>
		<rdfs:seeAlso rdf:resource="#OrgW3cDomLsLibrary"/>
		<rdfs:seeAlso rdf:resource="#JavaNetLibrary"/>
		<rdfs:seeAlso rdf:resource="#OrgXmlSaxLibrary"/>
		<rdfs:seeAlso rdf:resource="#JavaxXmlTransformLibrary"/>
		<rdfs:comment xml:lang="en">JavaLibrary implementing the javax.xml.validation package for j2se-1_5</rdfs:comment>
	</owl:Class>
	<owl:Class rdf:about="#JavaxXmlXpathLibrary">
		<rdfs:subClassOf rdf:resource="&java;JavaLibrary"/>
		<rdfs:seeAlso rdf:resource="#JavaIoLibrary"/>
		<rdfs:seeAlso rdf:resource="#JavaUtilLibrary"/>
		<rdfs:seeAlso rdf:resource="#JavaxXmlNamespaceLibrary"/>
		<rdfs:seeAlso rdf:resource="#JavaLangLibrary"/>
		<rdfs:seeAlso rdf:resource="#OrgXmlSaxLibrary"/>
		<rdfs:comment xml:lang="en">JavaLibrary implementing the javax.xml.xpath package for j2se-1_5</rdfs:comment>
	</owl:Class>
	<owl:Class rdf:about="#OrgW3cDomLibrary">
		<rdfs:subClassOf rdf:resource="&j2se-1_4;OrgW3cDomLibrary"/>
		<rdfs:seeAlso rdf:resource="#JavaLangLibrary"/>
		<rdfs:comment xml:lang="en">JavaLibrary implementing the org.w3c.dom package for j2se-1_5</rdfs:comment>
	</owl:Class>
	<owl:Class rdf:about="#OrgW3cDomBootstrapLibrary">
		<rdfs:subClassOf rdf:resource="&java;JavaLibrary"/>
		<rdfs:seeAlso rdf:resource="#OrgW3cDomLibrary"/>
		<rdfs:seeAlso rdf:resource="#JavaLangLibrary"/>
		<rdfs:comment xml:lang="en">JavaLibrary implementing the org.w3c.dom.bootstrap package for j2se-1_5</rdfs:comment>
	</owl:Class>
	<owl:Class rdf:about="#OrgW3cDomCssLibrary">
		<rdfs:subClassOf rdf:resource="&j2se-1_4;OrgW3cDomCssLibrary"/>
		<rdfs:seeAlso rdf:resource="#OrgW3cDomLibrary"/>
		<rdfs:seeAlso rdf:resource="#JavaLangLibrary"/>
		<rdfs:seeAlso rdf:resource="#OrgW3cDomViewsLibrary"/>
		<rdfs:seeAlso rdf:resource="#OrgW3cDomStylesheetsLibrary"/>
		<rdfs:comment xml:lang="en">JavaLibrary implementing the org.w3c.dom.css package for j2se-1_5</rdfs:comment>
	</owl:Class>
	<owl:Class rdf:about="#OrgW3cDomStylesheetsLibrary">
		<owl:equivalentClass rdf:resource="&j2se-1_4;OrgW3cDomStylesheetsLibrary"/>
		<rdfs:subClassOf rdf:resource="&java;JavaLibrary"/>
		<rdfs:seeAlso rdf:resource="#OrgW3cDomLibrary"/>
		<rdfs:seeAlso rdf:resource="#JavaLangLibrary"/>
		<rdfs:comment xml:lang="en">JavaLibrary implementing the org.w3c.dom.stylesheets package for j2se-1_5</rdfs:comment>
	</owl:Class>
	<owl:Class rdf:about="#OrgW3cDomViewsLibrary">
		<owl:equivalentClass rdf:resource="&j2se-1_4;OrgW3cDomViewsLibrary"/>
		<rdfs:subClassOf rdf:resource="&java;JavaLibrary"/>
		<rdfs:comment xml:lang="en">JavaLibrary implementing the org.w3c.dom.views package for j2se-1_5</rdfs:comment>
	</owl:Class>
	<owl:Class rdf:about="#OrgW3cDomEventsLibrary">
		<owl:equivalentClass rdf:resource="&j2se-1_4;OrgW3cDomEventsLibrary"/>
		<rdfs:subClassOf rdf:resource="&java;JavaLibrary"/>
		<rdfs:seeAlso rdf:resource="#OrgW3cDomLibrary"/>
		<rdfs:seeAlso rdf:resource="#JavaLangLibrary"/>
		<rdfs:seeAlso rdf:resource="#OrgW3cDomViewsLibrary"/>
		<rdfs:comment xml:lang="en">JavaLibrary implementing the org.w3c.dom.events package for j2se-1_5</rdfs:comment>
	</owl:Class>
	<owl:Class rdf:about="#OrgW3cDomHtmlLibrary">
		<rdfs:subClassOf rdf:resource="&j2se-1_4;OrgW3cDomHtmlLibrary"/>
		<rdfs:seeAlso rdf:resource="#OrgW3cDomLibrary"/>
		<rdfs:seeAlso rdf:resource="#JavaLangLibrary"/>
		<rdfs:comment xml:lang="en">JavaLibrary implementing the org.w3c.dom.html package for j2se-1_5</rdfs:comment>
	</owl:Class>
	<owl:Class rdf:about="#OrgW3cDomLsLibrary">
		<rdfs:subClassOf rdf:resource="&java;JavaLibrary"/>
		<rdfs:seeAlso rdf:resource="#JavaLangLibrary"/>
		<rdfs:seeAlso rdf:resource="#OrgW3cDomTraversalLibrary"/>
		<rdfs:seeAlso rdf:resource="#JavaIoLibrary"/>
		<rdfs:seeAlso rdf:resource="#OrgW3cDomLibrary"/>
		<rdfs:seeAlso rdf:resource="#OrgW3cDomEventsLibrary"/>
		<rdfs:comment xml:lang="en">JavaLibrary implementing the org.w3c.dom.ls package for j2se-1_5</rdfs:comment>
	</owl:Class>
	<owl:Class rdf:about="#OrgW3cDomTraversalLibrary">
		<owl:equivalentClass rdf:resource="&j2se-1_4;OrgW3cDomTraversalLibrary"/>
		<rdfs:subClassOf rdf:resource="&java;JavaLibrary"/>
		<rdfs:seeAlso rdf:resource="#OrgW3cDomLibrary"/>
		<rdfs:comment xml:lang="en">JavaLibrary implementing the org.w3c.dom.traversal package for j2se-1_5</rdfs:comment>
	</owl:Class>
	<owl:Class rdf:about="#OrgW3cDomRangesLibrary">
		<rdfs:subClassOf rdf:resource="&java;JavaLibrary"/>
		<rdfs:seeAlso rdf:resource="#OrgW3cDomLibrary"/>
		<rdfs:seeAlso rdf:resource="#JavaLangLibrary"/>
		<rdfs:comment xml:lang="en">JavaLibrary implementing the org.w3c.dom.ranges package for j2se-1_5</rdfs:comment>
	</owl:Class>
	<owl:Class rdf:about="#OrgOmgCORBA_2_3Library">
		<owl:equivalentClass rdf:resource="&j2se-1_4;OrgOmgCORBA_2_3Library"/>
		<rdfs:subClassOf rdf:resource="&java;JavaLibrary"/>
		<rdfs:seeAlso rdf:resource="#OrgOmgCORBALibrary"/>
		<rdfs:seeAlso rdf:resource="#JavaLangLibrary"/>
		<rdfs:seeAlso rdf:resource="#OrgOmgCORBAPortableLibrary"/>
		<rdfs:comment xml:lang="en">JavaLibrary implementing the org.omg.CORBA_2_3 package for j2se-1_5</rdfs:comment>
	</owl:Class>
	<owl:Class rdf:about="#OrgOmgCORBA_2_3PortableLibrary">
		<owl:equivalentClass rdf:resource="&j2se-1_4;OrgOmgCORBA_2_3PortableLibrary"/>
		<rdfs:subClassOf rdf:resource="&java;JavaLibrary"/>
		<rdfs:seeAlso rdf:resource="#JavaIoLibrary"/>
		<rdfs:seeAlso rdf:resource="#OrgOmgCORBALibrary"/>
		<rdfs:seeAlso rdf:resource="#JavaLangLibrary"/>
		<rdfs:seeAlso rdf:resource="#OrgOmgCORBAPortableLibrary"/>
		<rdfs:comment xml:lang="en">JavaLibrary implementing the org.omg.CORBA_2_3.portable package for j2se-1_5</rdfs:comment>
	</owl:Class>
	<owl:Class rdf:about="#OrgOmgCORBALibrary">
		<rdfs:subClassOf rdf:resource="&java;JavaLibrary"/>
		<rdfs:seeAlso rdf:resource="#JavaMathLibrary"/>
		<rdfs:seeAlso rdf:resource="#JavaUtilLibrary"/>
		<rdfs:seeAlso rdf:resource="#JavaLangLibrary"/>
		<rdfs:seeAlso rdf:resource="#JavaAppletLibrary"/>
		<rdfs:seeAlso rdf:resource="#OrgOmgCORBAPortableLibrary"/>
		<rdfs:seeAlso rdf:resource="#JavaIoLibrary"/>
		<rdfs:comment xml:lang="en">JavaLibrary implementing the org.omg.CORBA package for j2se-1_5</rdfs:comment>
	</owl:Class>
	<owl:Class rdf:about="#OrgOmgCORBAPortableLibrary">
		<rdfs:subClassOf rdf:resource="&j2se-1_4;OrgOmgCORBAPortableLibrary"/>
		<rdfs:seeAlso rdf:resource="#JavaMathLibrary"/>
		<rdfs:seeAlso rdf:resource="#OrgOmgCORBA_2_3PortableLibrary"/>
		<rdfs:seeAlso rdf:resource="#JavaIoLibrary"/>
		<rdfs:seeAlso rdf:resource="#OrgOmgCORBALibrary"/>
		<rdfs:seeAlso rdf:resource="#JavaLangLibrary"/>
		<rdfs:comment xml:lang="en">JavaLibrary implementing the org.omg.CORBA.portable package for j2se-1_5</rdfs:comment>
	</owl:Class>
	<owl:Class rdf:about="#OrgOmgCORBADynAnyPackageLibrary">
		<owl:equivalentClass rdf:resource="&j2se-1_4;OrgOmgCORBADynAnyPackageLibrary"/>
		<rdfs:subClassOf rdf:resource="&java;JavaLibrary"/>
		<rdfs:seeAlso rdf:resource="#OrgOmgCORBALibrary"/>
		<rdfs:seeAlso rdf:resource="#JavaLangLibrary"/>
		<rdfs:comment xml:lang="en">JavaLibrary implementing the org.omg.CORBA.DynAnyPackage package for j2se-1_5</rdfs:comment>
	</owl:Class>
	<owl:Class rdf:about="#OrgOmgCORBAORBPackageLibrary">
		<owl:equivalentClass rdf:resource="&j2se-1_4;OrgOmgCORBAORBPackageLibrary"/>
		<rdfs:subClassOf rdf:resource="&java;JavaLibrary"/>
		<rdfs:seeAlso rdf:resource="#OrgOmgCORBALibrary"/>
		<rdfs:seeAlso rdf:resource="#JavaLangLibrary"/>
		<rdfs:comment xml:lang="en">JavaLibrary implementing the org.omg.CORBA.ORBPackage package for j2se-1_5</rdfs:comment>
	</owl:Class>
	<owl:Class rdf:about="#OrgOmgCORBATypeCodePackageLibrary">
		<owl:equivalentClass rdf:resource="&j2se-1_4;OrgOmgCORBATypeCodePackageLibrary"/>
		<rdfs:subClassOf rdf:resource="&java;JavaLibrary"/>
		<rdfs:seeAlso rdf:resource="#OrgOmgCORBALibrary"/>
		<rdfs:seeAlso rdf:resource="#JavaLangLibrary"/>
		<rdfs:comment xml:lang="en">JavaLibrary implementing the org.omg.CORBA.TypeCodePackage package for j2se-1_5</rdfs:comment>
	</owl:Class>
	<owl:Class rdf:about="#OrgOmgCosNamingLibrary">
		<rdfs:subClassOf rdf:resource="&j2se-1_4;OrgOmgCosNamingLibrary"/>
		<rdfs:seeAlso rdf:resource="#JavaLangLibrary"/>
		<rdfs:seeAlso rdf:resource="#OrgOmgCORBAPortableLibrary"/>
		<rdfs:seeAlso rdf:resource="#OrgOmgCORBALibrary"/>
		<rdfs:seeAlso rdf:resource="#OrgOmgPortableServerLibrary"/>
		<rdfs:comment xml:lang="en">JavaLibrary implementing the org.omg.CosNaming package for j2se-1_5</rdfs:comment>
	</owl:Class>
	<owl:Class rdf:about="#OrgOmgCosNamingNamingContextExtPackageLibrary">
		<owl:equivalentClass rdf:resource="&j2se-1_4;OrgOmgCosNamingNamingContextExtPackageLibrary"/>
		<rdfs:subClassOf rdf:resource="&java;JavaLibrary"/>
		<rdfs:seeAlso rdf:resource="#OrgOmgCORBALibrary"/>
		<rdfs:seeAlso rdf:resource="#JavaLangLibrary"/>
		<rdfs:seeAlso rdf:resource="#OrgOmgCORBAPortableLibrary"/>
		<rdfs:comment xml:lang="en">JavaLibrary implementing the org.omg.CosNaming.NamingContextExtPackage package for j2se-1_5</rdfs:comment>
	</owl:Class>
	<owl:Class rdf:about="#OrgOmgCosNamingNamingContextPackageLibrary">
		<owl:equivalentClass rdf:resource="&j2se-1_4;OrgOmgCosNamingNamingContextPackageLibrary"/>
		<rdfs:subClassOf rdf:resource="&java;JavaLibrary"/>
		<rdfs:seeAlso rdf:resource="#OrgOmgCORBALibrary"/>
		<rdfs:seeAlso rdf:resource="#JavaLangLibrary"/>
		<rdfs:seeAlso rdf:resource="#OrgOmgCosNamingLibrary"/>
		<rdfs:seeAlso rdf:resource="#OrgOmgCORBAPortableLibrary"/>
		<rdfs:comment xml:lang="en">JavaLibrary implementing the org.omg.CosNaming.NamingContextPackage package for j2se-1_5</rdfs:comment>
	</owl:Class>
	<owl:Class rdf:about="#OrgOmgPortableServerLibrary">
		<rdfs:subClassOf rdf:resource="&j2se-1_4;OrgOmgPortableServerLibrary"/>
		<rdfs:seeAlso rdf:resource="#OrgOmgPortableServerPOAManagerPackageLibrary"/>
		<rdfs:seeAlso rdf:resource="#JavaLangLibrary"/>
		<rdfs:seeAlso rdf:resource="#OrgOmgCORBAPortableLibrary"/>
		<rdfs:seeAlso rdf:resource="#OrgOmgPortableServerPortableLibrary"/>
		<rdfs:seeAlso rdf:resource="#OrgOmgCORBALibrary"/>
		<rdfs:seeAlso rdf:resource="#OrgOmgPortableServerServantLocatorPackageLibrary"/>
		<rdfs:comment xml:lang="en">JavaLibrary implementing the org.omg.PortableServer package for j2se-1_5</rdfs:comment>
	</owl:Class>
	<owl:Class rdf:about="#OrgOmgPortableServerCurrentPackageLibrary">
		<owl:equivalentClass rdf:resource="&j2se-1_4;OrgOmgPortableServerCurrentPackageLibrary"/>
		<rdfs:subClassOf rdf:resource="&java;JavaLibrary"/>
		<rdfs:seeAlso rdf:resource="#OrgOmgCORBALibrary"/>
		<rdfs:seeAlso rdf:resource="#JavaLangLibrary"/>
		<rdfs:seeAlso rdf:resource="#OrgOmgCORBAPortableLibrary"/>
		<rdfs:comment xml:lang="en">JavaLibrary implementing the org.omg.PortableServer.CurrentPackage package for j2se-1_5</rdfs:comment>
	</owl:Class>
	<owl:Class rdf:about="#OrgOmgPortableServerPOAManagerPackageLibrary">
		<owl:equivalentClass rdf:resource="&j2se-1_4;OrgOmgPortableServerPOAManagerPackageLibrary"/>
		<rdfs:subClassOf rdf:resource="&java;JavaLibrary"/>
		<rdfs:seeAlso rdf:resource="#OrgOmgCORBALibrary"/>
		<rdfs:seeAlso rdf:resource="#JavaLangLibrary"/>
		<rdfs:seeAlso rdf:resource="#OrgOmgCORBAPortableLibrary"/>
		<rdfs:comment xml:lang="en">JavaLibrary implementing the org.omg.PortableServer.POAManagerPackage package for j2se-1_5</rdfs:comment>
	</owl:Class>
	<owl:Class rdf:about="#OrgOmgPortableServerPOAPackageLibrary">
		<owl:equivalentClass rdf:resource="&j2se-1_4;OrgOmgPortableServerPOAPackageLibrary"/>
		<rdfs:subClassOf rdf:resource="&java;JavaLibrary"/>
		<rdfs:seeAlso rdf:resource="#OrgOmgCORBALibrary"/>
		<rdfs:seeAlso rdf:resource="#JavaLangLibrary"/>
		<rdfs:seeAlso rdf:resource="#OrgOmgCORBAPortableLibrary"/>
		<rdfs:comment xml:lang="en">JavaLibrary implementing the org.omg.PortableServer.POAPackage package for j2se-1_5</rdfs:comment>
	</owl:Class>
	<owl:Class rdf:about="#OrgOmgPortableServerServantLocatorPackageLibrary">
		<owl:equivalentClass rdf:resource="&j2se-1_4;OrgOmgPortableServerServantLocatorPackageLibrary"/>
		<rdfs:subClassOf rdf:resource="&java;JavaLibrary"/>
		<rdfs:seeAlso rdf:resource="#OrgOmgCORBALibrary"/>
		<rdfs:seeAlso rdf:resource="#JavaLangLibrary"/>
		<rdfs:seeAlso rdf:resource="#OrgOmgCORBAPortableLibrary"/>
		<rdfs:comment xml:lang="en">JavaLibrary implementing the org.omg.PortableServer.ServantLocatorPackage package for j2se-1_5</rdfs:comment>
	</owl:Class>
	<owl:Class rdf:about="#OrgOmgPortableServerPortableLibrary">
		<owl:equivalentClass rdf:resource="&j2se-1_4;OrgOmgPortableServerPortableLibrary"/>
		<rdfs:subClassOf rdf:resource="&java;JavaLibrary"/>
		<rdfs:seeAlso rdf:resource="#OrgOmgCORBALibrary"/>
		<rdfs:seeAlso rdf:resource="#JavaLangLibrary"/>
		<rdfs:seeAlso rdf:resource="#OrgOmgPortableServerLibrary"/>
		<rdfs:comment xml:lang="en">JavaLibrary implementing the org.omg.PortableServer.portable package for j2se-1_5</rdfs:comment>
	</owl:Class>
	<owl:Class rdf:about="#OrgOmgDynamicLibrary">
		<owl:equivalentClass rdf:resource="&j2se-1_4;OrgOmgDynamicLibrary"/>
		<rdfs:subClassOf rdf:resource="&java;JavaLibrary"/>
		<rdfs:seeAlso rdf:resource="#OrgOmgCORBALibrary"/>
		<rdfs:seeAlso rdf:resource="#JavaLangLibrary"/>
		<rdfs:seeAlso rdf:resource="#OrgOmgCORBAPortableLibrary"/>
		<rdfs:comment xml:lang="en">JavaLibrary implementing the org.omg.Dynamic package for j2se-1_5</rdfs:comment>
	</owl:Class>
	<owl:Class rdf:about="#OrgOmgDynamicAnyLibrary">
		<rdfs:subClassOf rdf:resource="&j2se-1_4;OrgOmgDynamicAnyLibrary"/>
		<rdfs:seeAlso rdf:resource="#JavaLangLibrary"/>
		<rdfs:seeAlso rdf:resource="#OrgOmgCORBAPortableLibrary"/>
		<rdfs:seeAlso rdf:resource="#JavaIoLibrary"/>
		<rdfs:seeAlso rdf:resource="#OrgOmgCORBALibrary"/>
		<rdfs:comment xml:lang="en">JavaLibrary implementing the org.omg.DynamicAny package for j2se-1_5</rdfs:comment>
	</owl:Class>
	<owl:Class rdf:about="#OrgOmgDynamicAnyDynAnyFactoryPackageLibrary">
		<owl:equivalentClass rdf:resource="&j2se-1_4;OrgOmgDynamicAnyDynAnyFactoryPackageLibrary"/>
		<rdfs:subClassOf rdf:resource="&java;JavaLibrary"/>
		<rdfs:seeAlso rdf:resource="#OrgOmgCORBALibrary"/>
		<rdfs:seeAlso rdf:resource="#JavaLangLibrary"/>
		<rdfs:seeAlso rdf:resource="#OrgOmgCORBAPortableLibrary"/>
		<rdfs:comment xml:lang="en">JavaLibrary implementing the org.omg.DynamicAny.DynAnyFactoryPackage package for j2se-1_5</rdfs:comment>
	</owl:Class>
	<owl:Class rdf:about="#OrgOmgDynamicAnyDynAnyPackageLibrary">
		<owl:equivalentClass rdf:resource="&j2se-1_4;OrgOmgDynamicAnyDynAnyPackageLibrary"/>
		<rdfs:subClassOf rdf:resource="&java;JavaLibrary"/>
		<rdfs:seeAlso rdf:resource="#OrgOmgCORBALibrary"/>
		<rdfs:seeAlso rdf:resource="#JavaLangLibrary"/>
		<rdfs:seeAlso rdf:resource="#OrgOmgCORBAPortableLibrary"/>
		<rdfs:comment xml:lang="en">JavaLibrary implementing the org.omg.DynamicAny.DynAnyPackage package for j2se-1_5</rdfs:comment>
	</owl:Class>
	<owl:Class rdf:about="#OrgOmgIOPLibrary">
		<rdfs:subClassOf rdf:resource="&j2se-1_4;OrgOmgIOPLibrary"/>
		<rdfs:seeAlso rdf:resource="#OrgOmgCORBALibrary"/>
		<rdfs:seeAlso rdf:resource="#JavaLangLibrary"/>
		<rdfs:seeAlso rdf:resource="#OrgOmgCORBAPortableLibrary"/>
		<rdfs:comment xml:lang="en">JavaLibrary implementing the org.omg.IOP package for j2se-1_5</rdfs:comment>
	</owl:Class>
	<owl:Class rdf:about="#OrgOmgIOPCodecFactoryPackageLibrary">
		<owl:equivalentClass rdf:resource="&j2se-1_4;OrgOmgIOPCodecFactoryPackageLibrary"/>
		<rdfs:subClassOf rdf:resource="&java;JavaLibrary"/>
		<rdfs:seeAlso rdf:resource="#OrgOmgCORBALibrary"/>
		<rdfs:seeAlso rdf:resource="#JavaLangLibrary"/>
		<rdfs:seeAlso rdf:resource="#OrgOmgCORBAPortableLibrary"/>
		<rdfs:comment xml:lang="en">JavaLibrary implementing the org.omg.IOP.CodecFactoryPackage package for j2se-1_5</rdfs:comment>
	</owl:Class>
	<owl:Class rdf:about="#OrgOmgIOPCodecPackageLibrary">
		<owl:equivalentClass rdf:resource="&j2se-1_4;OrgOmgIOPCodecPackageLibrary"/>
		<rdfs:subClassOf rdf:resource="&java;JavaLibrary"/>
		<rdfs:seeAlso rdf:resource="#OrgOmgCORBALibrary"/>
		<rdfs:seeAlso rdf:resource="#JavaLangLibrary"/>
		<rdfs:seeAlso rdf:resource="#OrgOmgCORBAPortableLibrary"/>
		<rdfs:comment xml:lang="en">JavaLibrary implementing the org.omg.IOP.CodecPackage package for j2se-1_5</rdfs:comment>
	</owl:Class>
	<owl:Class rdf:about="#OrgOmgMessagingLibrary">
		<owl:equivalentClass rdf:resource="&j2se-1_4;OrgOmgMessagingLibrary"/>
		<rdfs:subClassOf rdf:resource="&java;JavaLibrary"/>
		<rdfs:seeAlso rdf:resource="#OrgOmgCORBALibrary"/>
		<rdfs:seeAlso rdf:resource="#JavaLangLibrary"/>
		<rdfs:seeAlso rdf:resource="#OrgOmgCORBAPortableLibrary"/>
		<rdfs:comment xml:lang="en">JavaLibrary implementing the org.omg.Messaging package for j2se-1_5</rdfs:comment>
	</owl:Class>
	<owl:Class rdf:about="#OrgOmgPortableInterceptorLibrary">
		<rdfs:subClassOf rdf:resource="&j2se-1_4;OrgOmgPortableInterceptorLibrary"/>
		<rdfs:seeAlso rdf:resource="#JavaLangLibrary"/>
		<rdfs:seeAlso rdf:resource="#OrgOmgIOPLibrary"/>
		<rdfs:seeAlso rdf:resource="#OrgOmgCORBAPortableLibrary"/>
		<rdfs:seeAlso rdf:resource="#OrgOmgCORBALibrary"/>
		<rdfs:comment xml:lang="en">JavaLibrary implementing the org.omg.PortableInterceptor package for j2se-1_5</rdfs:comment>
	</owl:Class>
	<owl:Class rdf:about="#OrgOmgPortableInterceptorORBInitInfoPackageLibrary">
		<owl:equivalentClass rdf:resource="&j2se-1_4;OrgOmgPortableInterceptorORBInitInfoPackageLibrary"/>
		<rdfs:subClassOf rdf:resource="&java;JavaLibrary"/>
		<rdfs:seeAlso rdf:resource="#OrgOmgCORBALibrary"/>
		<rdfs:seeAlso rdf:resource="#JavaLangLibrary"/>
		<rdfs:seeAlso rdf:resource="#OrgOmgCORBAPortableLibrary"/>
		<rdfs:comment xml:lang="en">JavaLibrary implementing the org.omg.PortableInterceptor.ORBInitInfoPackage package for j2se-1_5</rdfs:comment>
	</owl:Class>
	<owl:Class rdf:about="#OrgOmgSendingContextLibrary">
		<owl:equivalentClass rdf:resource="&j2se-1_4;OrgOmgSendingContextLibrary"/>
		<rdfs:subClassOf rdf:resource="&java;JavaLibrary"/>
		<rdfs:seeAlso rdf:resource="#OrgOmgCORBALibrary"/>
		<rdfs:seeAlso rdf:resource="#OrgOmgCORBAPortableLibrary"/>
		<rdfs:comment xml:lang="en">JavaLibrary implementing the org.omg.SendingContext package for j2se-1_5</rdfs:comment>
	</owl:Class>
	<owl:Class rdf:about="#OrgOmgStubJavaRmiLibrary">
		<owl:equivalentClass rdf:resource="&j2se-1_4;OrgOmgStubJavaRmiLibrary"/>
		<rdfs:subClassOf rdf:resource="&java;JavaLibrary"/>
		<rdfs:seeAlso rdf:resource="#JavaxRmiCORBALibrary"/>
		<rdfs:seeAlso rdf:resource="#JavaRmiLibrary"/>
		<rdfs:comment xml:lang="en">JavaLibrary implementing the org.omg.stub.java.rmi package for j2se-1_5</rdfs:comment>
	</owl:Class>
	<owl:Class rdf:about="#OrgOmgStubJavaxManagementRemoteRmiLibrary">
		<rdfs:subClassOf rdf:resource="&java;JavaLibrary"/>
		<rdfs:seeAlso rdf:resource="#JavaxManagementRemoteLibrary"/>
		<rdfs:seeAlso rdf:resource="#JavaxSecurityAuthLibrary"/>
		<rdfs:seeAlso rdf:resource="#JavaUtilLibrary"/>
		<rdfs:seeAlso rdf:resource="#JavaLangLibrary"/>
		<rdfs:seeAlso rdf:resource="#JavaxRmiCORBALibrary"/>
		<rdfs:seeAlso rdf:resource="#OrgOmgCORBAPortableLibrary"/>
		<rdfs:seeAlso rdf:resource="#JavaRmiLibrary"/>
		<rdfs:seeAlso rdf:resource="#OrgOmgCORBA_2_3PortableLibrary"/>
		<rdfs:seeAlso rdf:resource="#OrgOmgCORBALibrary"/>
		<rdfs:seeAlso rdf:resource="#JavaxManagementRemoteRmiLibrary"/>
		<rdfs:seeAlso rdf:resource="#JavaxManagementLibrary"/>
		<rdfs:comment xml:lang="en">JavaLibrary implementing the org.omg.stub.javax.management.remote.rmi package for j2se-1_5</rdfs:comment>
	</owl:Class>
	<owl:Class rdf:about="#OrgXmlSaxLibrary">
		<owl:equivalentClass rdf:resource="&j2se-1_4;OrgXmlSaxLibrary"/>
		<rdfs:subClassOf rdf:resource="&java;JavaLibrary"/>
		<rdfs:seeAlso rdf:resource="#JavaIoLibrary"/>
		<rdfs:seeAlso rdf:resource="#JavaUtilLibrary"/>
		<rdfs:seeAlso rdf:resource="#JavaLangLibrary"/>
		<rdfs:comment xml:lang="en">JavaLibrary implementing the org.xml.sax package for j2se-1_5</rdfs:comment>
	</owl:Class>
	<owl:Class rdf:about="#OrgXmlSaxExtLibrary">
		<rdfs:subClassOf rdf:resource="&j2se-1_4;OrgXmlSaxExtLibrary"/>
		<rdfs:seeAlso rdf:resource="#JavaLangLibrary"/>
		<rdfs:seeAlso rdf:resource="#OrgXmlSaxHelpersLibrary"/>
		<rdfs:seeAlso rdf:resource="#OrgXmlSaxLibrary"/>
		<rdfs:comment xml:lang="en">JavaLibrary implementing the org.xml.sax.ext package for j2se-1_5</rdfs:comment>
	</owl:Class>
	<owl:Class rdf:about="#OrgXmlSaxHelpersLibrary">
		<rdfs:subClassOf rdf:resource="&j2se-1_4;OrgXmlSaxHelpersLibrary"/>
		<rdfs:seeAlso rdf:resource="#JavaUtilLibrary"/>
		<rdfs:seeAlso rdf:resource="#JavaLangLibrary"/>
		<rdfs:seeAlso rdf:resource="#OrgXmlSaxLibrary"/>
		<rdfs:comment xml:lang="en">JavaLibrary implementing the org.xml.sax.helpers package for j2se-1_5</rdfs:comment>
	</owl:Class>
	<owl:Class rdf:about="#OrgIetfJgssLibrary">
		<owl:equivalentClass rdf:resource="&j2se-1_4;OrgIetfJgssLibrary"/>
		<rdfs:subClassOf rdf:resource="&java;JavaLibrary"/>
		<rdfs:seeAlso rdf:resource="#JavaIoLibrary"/>
		<rdfs:seeAlso rdf:resource="#JavaSecurityLibrary"/>
		<rdfs:seeAlso rdf:resource="#JavaLangLibrary"/>
		<rdfs:seeAlso rdf:resource="#JavaNetLibrary"/>
		<rdfs:comment xml:lang="en">JavaLibrary implementing the org.ietf.jgss package for j2se-1_5</rdfs:comment>
	</owl:Class>
</rdf:RDF>
