<?xml version="1.0" encoding="ISO-8859-1"?>
<!DOCTYPE rdf:RDF [
	<!ENTITY xsd "http://www.w3.org/2001/XMLSchema#">
	<!ENTITY owl "http://www.w3.org/2002/07/owl#">
	<!ENTITY rdfs "http://www.w3.org/2000/01/rdf-schema#">
	<!ENTITY rdf "http://www.w3.org/1999/02/22-rdf-syntax-ns#">
	<!ENTITY units "http://www.cs.kuleuven.be/~distrinet/projects/CoDAMoS/2005/01/Units.owl#">
	<!ENTITY platform "http://www.cs.kuleuven.be/~distrinet/projects/CoDAMoS/2007/01/Platform.owl#">
	<!ENTITY java "http://ssel.vub.ac.be/codamos/2007/01/Java.owl#">
	<!ENTITY j2se-1_5 "http://ssel.vub.ac.be/codamos/2007/01/j2se-1_5-api.owl#">
	<!ENTITY DEFAULT "http://ssel.vub.ac.be/codamos/2007/01/j2se-1_6-api.owl">
]>
<rdf:RDF
	 xmlns:xsd="&xsd;"
	 xmlns:owl="&owl;"
	 xmlns:rdfs="&rdfs;"
	 xmlns:rdf="&rdf;"
	 xmlns:units="&units;"
	 xmlns:platform="&platform;"
	 xmlns:java="&java;"
	 xmlns:j2se-1_5="&j2se-1_5;"
	 xmlns = "&DEFAULT;#"
	 xml:base = "&DEFAULT;"
>

	<owl:Ontology rdf:about="">
		<owl:imports rdf:resource="http://www.cs.kuleuven.be/~distrinet/projects/CoDAMoS/2007/01/Platform.owl"/>
		<owl:imports rdf:resource="http://ssel.vub.ac.be/codamos/2007/01/Java.owl"/>
		<owl:imports rdf:resource="http://ssel.vub.ac.be/codamos/2007/01/j2se-1_5-api.owl"/>
		<rdfs:comment xml:lang="en">Generated by $Id: UML2ToPackageAPIOntology.atl 7062 2007-06-30 11:16:05Z dwagelaa $ and $Id: UML2ToAPIOntology.atl 7062 2007-06-30 11:16:05Z dwagelaa $ and $Id:UML2Comparison.atl 7084 2007-07-10 13:19:05Z dwagelaa $</rdfs:comment>
		<rdfs:label xml:lang="en">j2se-1_6</rdfs:label>
	</owl:Ontology>
	<owl:Class rdf:about="#J2se-1_6ClassLibrary">
		<rdfs:subClassOf rdf:resource="#JavaAppletLibrary"/>
		<rdfs:subClassOf rdf:resource="#JavaAwtLibrary"/>
		<rdfs:subClassOf rdf:resource="#JavaAwtEventLibrary"/>
		<rdfs:subClassOf rdf:resource="#JavaAwtColorLibrary"/>
		<rdfs:subClassOf rdf:resource="#JavaAwtDatatransferLibrary"/>
		<rdfs:subClassOf rdf:resource="#JavaAwtDndLibrary"/>
		<rdfs:subClassOf rdf:resource="#JavaAwtDndPeerLibrary"/>
		<rdfs:subClassOf rdf:resource="#JavaAwtFontLibrary"/>
		<rdfs:subClassOf rdf:resource="#JavaAwtGeomLibrary"/>
		<rdfs:subClassOf rdf:resource="#JavaAwtImLibrary"/>
		<rdfs:subClassOf rdf:resource="#JavaAwtImSpiLibrary"/>
		<rdfs:subClassOf rdf:resource="#JavaAwtImageLibrary"/>
		<rdfs:subClassOf rdf:resource="#JavaAwtImageRenderableLibrary"/>
		<rdfs:subClassOf rdf:resource="#JavaAwtPeerLibrary"/>
		<rdfs:subClassOf rdf:resource="#JavaAwtPrintLibrary"/>
		<rdfs:subClassOf rdf:resource="#JavaLangLibrary"/>
		<rdfs:subClassOf rdf:resource="#JavaLangAnnotationLibrary"/>
		<rdfs:subClassOf rdf:resource="#JavaLangReflectLibrary"/>
		<rdfs:subClassOf rdf:resource="#JavaLangInstrumentLibrary"/>
		<rdfs:subClassOf rdf:resource="#JavaLangManagementLibrary"/>
		<rdfs:subClassOf rdf:resource="#JavaLangRefLibrary"/>
		<rdfs:subClassOf rdf:resource="#JavaIoLibrary"/>
		<rdfs:subClassOf rdf:resource="#JavaUtilLibrary"/>
		<rdfs:subClassOf rdf:resource="#JavaUtilSpiLibrary"/>
		<rdfs:subClassOf rdf:resource="#JavaUtilConcurrentLibrary"/>
		<rdfs:subClassOf rdf:resource="#JavaUtilConcurrentAtomicLibrary"/>
		<rdfs:subClassOf rdf:resource="#JavaUtilConcurrentLocksLibrary"/>
		<rdfs:subClassOf rdf:resource="#JavaUtilJarLibrary"/>
		<rdfs:subClassOf rdf:resource="#JavaUtilZipLibrary"/>
		<rdfs:subClassOf rdf:resource="#JavaUtilLoggingLibrary"/>
		<rdfs:subClassOf rdf:resource="#JavaUtilPrefsLibrary"/>
		<rdfs:subClassOf rdf:resource="#JavaUtilRegexLibrary"/>
		<rdfs:subClassOf rdf:resource="#JavaBeansLibrary"/>
		<rdfs:subClassOf rdf:resource="#JavaBeansBeancontextLibrary"/>
		<rdfs:subClassOf rdf:resource="#JavaSecurityLibrary"/>
		<rdfs:subClassOf rdf:resource="#JavaSecurityAclLibrary"/>
		<rdfs:subClassOf rdf:resource="#JavaSecurityCertLibrary"/>
		<rdfs:subClassOf rdf:resource="#JavaSecurityInterfacesLibrary"/>
		<rdfs:subClassOf rdf:resource="#JavaSecuritySpecLibrary"/>
		<rdfs:subClassOf rdf:resource="#JavaMathLibrary"/>
		<rdfs:subClassOf rdf:resource="#JavaNetLibrary"/>
		<rdfs:subClassOf rdf:resource="#JavaNioLibrary"/>
		<rdfs:subClassOf rdf:resource="#JavaNioChannelsLibrary"/>
		<rdfs:subClassOf rdf:resource="#JavaNioChannelsSpiLibrary"/>
		<rdfs:subClassOf rdf:resource="#JavaNioCharsetLibrary"/>
		<rdfs:subClassOf rdf:resource="#JavaNioCharsetSpiLibrary"/>
		<rdfs:subClassOf rdf:resource="#JavaRmiLibrary"/>
		<rdfs:subClassOf rdf:resource="#JavaRmiActivationLibrary"/>
		<rdfs:subClassOf rdf:resource="#JavaRmiServerLibrary"/>
		<rdfs:subClassOf rdf:resource="#JavaRmiDgcLibrary"/>
		<rdfs:subClassOf rdf:resource="#JavaRmiRegistryLibrary"/>
		<rdfs:subClassOf rdf:resource="#JavaSqlLibrary"/>
		<rdfs:subClassOf rdf:resource="#JavaTextLibrary"/>
		<rdfs:subClassOf rdf:resource="#JavaTextSpiLibrary"/>
		<rdfs:subClassOf rdf:resource="#JavaxAccessibilityLibrary"/>
		<rdfs:subClassOf rdf:resource="#JavaxSecurityAuthLibrary"/>
		<rdfs:subClassOf rdf:resource="#JavaxSecurityAuthLoginLibrary"/>
		<rdfs:subClassOf rdf:resource="#JavaxSecurityAuthCallbackLibrary"/>
		<rdfs:subClassOf rdf:resource="#JavaxSecurityAuthKerberosLibrary"/>
		<rdfs:subClassOf rdf:resource="#JavaxSecurityAuthSpiLibrary"/>
		<rdfs:subClassOf rdf:resource="#JavaxSecurityAuthX500Library"/>
		<rdfs:subClassOf rdf:resource="#JavaxSecuritySaslLibrary"/>
		<rdfs:subClassOf rdf:resource="#JavaxActivationLibrary"/>
		<rdfs:subClassOf rdf:resource="#JavaxActivityLibrary"/>
		<rdfs:subClassOf rdf:resource="#JavaxAnnotationLibrary"/>
		<rdfs:subClassOf rdf:resource="#JavaxAnnotationProcessingLibrary"/>
		<rdfs:subClassOf rdf:resource="#JavaxImageioLibrary"/>
		<rdfs:subClassOf rdf:resource="#JavaxImageioEventLibrary"/>
		<rdfs:subClassOf rdf:resource="#JavaxImageioMetadataLibrary"/>
		<rdfs:subClassOf rdf:resource="#JavaxImageioPluginsBmpLibrary"/>
		<rdfs:subClassOf rdf:resource="#JavaxImageioPluginsJpegLibrary"/>
		<rdfs:subClassOf rdf:resource="#JavaxImageioSpiLibrary"/>
		<rdfs:subClassOf rdf:resource="#JavaxImageioStreamLibrary"/>
		<rdfs:subClassOf rdf:resource="#JavaxJwsLibrary"/>
		<rdfs:subClassOf rdf:resource="#JavaxJwsSoapLibrary"/>
		<rdfs:subClassOf rdf:resource="#JavaxLangModelLibrary"/>
		<rdfs:subClassOf rdf:resource="#JavaxLangModelElementLibrary"/>
		<rdfs:subClassOf rdf:resource="#JavaxLangModelTypeLibrary"/>
		<rdfs:subClassOf rdf:resource="#JavaxLangModelUtilLibrary"/>
		<rdfs:subClassOf rdf:resource="#JavaxManagementLibrary"/>
		<rdfs:subClassOf rdf:resource="#JavaxManagementLoadingLibrary"/>
		<rdfs:subClassOf rdf:resource="#JavaxManagementModelmbeanLibrary"/>
		<rdfs:subClassOf rdf:resource="#JavaxManagementMonitorLibrary"/>
		<rdfs:subClassOf rdf:resource="#JavaxManagementOpenmbeanLibrary"/>
		<rdfs:subClassOf rdf:resource="#JavaxManagementRelationLibrary"/>
		<rdfs:subClassOf rdf:resource="#JavaxManagementRemoteLibrary"/>
		<rdfs:subClassOf rdf:resource="#JavaxManagementRemoteRmiLibrary"/>
		<rdfs:subClassOf rdf:resource="#JavaxManagementTimerLibrary"/>
		<rdfs:subClassOf rdf:resource="#JavaxRmiLibrary"/>
		<rdfs:subClassOf rdf:resource="#JavaxRmiCORBALibrary"/>
		<rdfs:subClassOf rdf:resource="#JavaxRmiSslLibrary"/>
		<rdfs:subClassOf rdf:resource="#JavaxNamingLibrary"/>
		<rdfs:subClassOf rdf:resource="#JavaxNamingDirectoryLibrary"/>
		<rdfs:subClassOf rdf:resource="#JavaxNamingEventLibrary"/>
		<rdfs:subClassOf rdf:resource="#JavaxNamingLdapLibrary"/>
		<rdfs:subClassOf rdf:resource="#JavaxNamingSpiLibrary"/>
		<rdfs:subClassOf rdf:resource="#JavaxPrintLibrary"/>
		<rdfs:subClassOf rdf:resource="#JavaxPrintAttributeLibrary"/>
		<rdfs:subClassOf rdf:resource="#JavaxPrintAttributeStandardLibrary"/>
		<rdfs:subClassOf rdf:resource="#JavaxPrintEventLibrary"/>
		<rdfs:subClassOf rdf:resource="#JavaxScriptLibrary"/>
		<rdfs:subClassOf rdf:resource="#JavaxCryptoLibrary"/>
		<rdfs:subClassOf rdf:resource="#JavaxSmartcardioLibrary"/>
		<rdfs:subClassOf rdf:resource="#JavaxSoundMidiLibrary"/>
		<rdfs:subClassOf rdf:resource="#JavaxSoundMidiSpiLibrary"/>
		<rdfs:subClassOf rdf:resource="#JavaxSoundSampledLibrary"/>
		<rdfs:subClassOf rdf:resource="#JavaxSoundSampledSpiLibrary"/>
		<rdfs:subClassOf rdf:resource="#JavaxSqlLibrary"/>
		<rdfs:subClassOf rdf:resource="#JavaxSqlRowsetLibrary"/>
		<rdfs:subClassOf rdf:resource="#JavaxSqlRowsetSerialLibrary"/>
		<rdfs:subClassOf rdf:resource="#JavaxSqlRowsetSpiLibrary"/>
		<rdfs:subClassOf rdf:resource="#JavaxSwingLibrary"/>
		<rdfs:subClassOf rdf:resource="#JavaxSwingEventLibrary"/>
		<rdfs:subClassOf rdf:resource="#JavaxSwingTextLibrary"/>
		<rdfs:subClassOf rdf:resource="#JavaxSwingTextHtmlLibrary"/>
		<rdfs:subClassOf rdf:resource="#JavaxSwingTextHtmlParserLibrary"/>
		<rdfs:subClassOf rdf:resource="#JavaxSwingTextRtfLibrary"/>
		<rdfs:subClassOf rdf:resource="#JavaxSwingTreeLibrary"/>
		<rdfs:subClassOf rdf:resource="#JavaxSwingBorderLibrary"/>
		<rdfs:subClassOf rdf:resource="#JavaxSwingColorchooserLibrary"/>
		<rdfs:subClassOf rdf:resource="#JavaxSwingFilechooserLibrary"/>
		<rdfs:subClassOf rdf:resource="#JavaxSwingPlafLibrary"/>
		<rdfs:subClassOf rdf:resource="#JavaxSwingPlafBasicLibrary"/>
		<rdfs:subClassOf rdf:resource="#JavaxSwingPlafMetalLibrary"/>
		<rdfs:subClassOf rdf:resource="#JavaxSwingPlafMultiLibrary"/>
		<rdfs:subClassOf rdf:resource="#JavaxSwingPlafSynthLibrary"/>
		<rdfs:subClassOf rdf:resource="#JavaxSwingTableLibrary"/>
		<rdfs:subClassOf rdf:resource="#JavaxSwingUndoLibrary"/>
		<rdfs:subClassOf rdf:resource="#JavaxToolsLibrary"/>
		<rdfs:subClassOf rdf:resource="#JavaxTransactionLibrary"/>
		<rdfs:subClassOf rdf:resource="#JavaxTransactionXaLibrary"/>
		<rdfs:subClassOf rdf:resource="#JavaxXmlLibrary"/>
		<rdfs:subClassOf rdf:resource="#JavaxXmlBindLibrary"/>
		<rdfs:subClassOf rdf:resource="#JavaxXmlBindAnnotationLibrary"/>
		<rdfs:subClassOf rdf:resource="#JavaxXmlBindAnnotationAdaptersLibrary"/>
		<rdfs:subClassOf rdf:resource="#JavaxXmlBindAttachmentLibrary"/>
		<rdfs:subClassOf rdf:resource="#JavaxXmlBindHelpersLibrary"/>
		<rdfs:subClassOf rdf:resource="#JavaxXmlBindUtilLibrary"/>
		<rdfs:subClassOf rdf:resource="#JavaxXmlTransformLibrary"/>
		<rdfs:subClassOf rdf:resource="#JavaxXmlTransformSaxLibrary"/>
		<rdfs:subClassOf rdf:resource="#JavaxXmlTransformDomLibrary"/>
		<rdfs:subClassOf rdf:resource="#JavaxXmlTransformStaxLibrary"/>
		<rdfs:subClassOf rdf:resource="#JavaxXmlTransformStreamLibrary"/>
		<rdfs:subClassOf rdf:resource="#JavaxXmlCryptoLibrary"/>
		<rdfs:subClassOf rdf:resource="#JavaxXmlCryptoDomLibrary"/>
		<rdfs:subClassOf rdf:resource="#JavaxXmlCryptoDsigLibrary"/>
		<rdfs:subClassOf rdf:resource="#JavaxXmlCryptoDsigDomLibrary"/>
		<rdfs:subClassOf rdf:resource="#JavaxXmlCryptoDsigKeyinfoLibrary"/>
		<rdfs:subClassOf rdf:resource="#JavaxXmlCryptoDsigSpecLibrary"/>
		<rdfs:subClassOf rdf:resource="#JavaxXmlDatatypeLibrary"/>
		<rdfs:subClassOf rdf:resource="#JavaxXmlNamespaceLibrary"/>
		<rdfs:subClassOf rdf:resource="#JavaxXmlParsersLibrary"/>
		<rdfs:subClassOf rdf:resource="#JavaxXmlSoapLibrary"/>
		<rdfs:subClassOf rdf:resource="#JavaxXmlStreamLibrary"/>
		<rdfs:subClassOf rdf:resource="#JavaxXmlStreamUtilLibrary"/>
		<rdfs:subClassOf rdf:resource="#JavaxXmlStreamEventsLibrary"/>
		<rdfs:subClassOf rdf:resource="#JavaxXmlValidationLibrary"/>
		<rdfs:subClassOf rdf:resource="#JavaxXmlWsLibrary"/>
		<rdfs:subClassOf rdf:resource="#JavaxXmlWsHandlerLibrary"/>
		<rdfs:subClassOf rdf:resource="#JavaxXmlWsHandlerSoapLibrary"/>
		<rdfs:subClassOf rdf:resource="#JavaxXmlWsHttpLibrary"/>
		<rdfs:subClassOf rdf:resource="#JavaxXmlWsSoapLibrary"/>
		<rdfs:subClassOf rdf:resource="#JavaxXmlWsSpiLibrary"/>
		<rdfs:subClassOf rdf:resource="#JavaxXmlXpathLibrary"/>
		<rdfs:subClassOf rdf:resource="#OrgW3cDomLibrary"/>
		<rdfs:subClassOf rdf:resource="#OrgW3cDomBootstrapLibrary"/>
		<rdfs:subClassOf rdf:resource="#OrgW3cDomCssLibrary"/>
		<rdfs:subClassOf rdf:resource="#OrgW3cDomStylesheetsLibrary"/>
		<rdfs:subClassOf rdf:resource="#OrgW3cDomViewsLibrary"/>
		<rdfs:subClassOf rdf:resource="#OrgW3cDomEventsLibrary"/>
		<rdfs:subClassOf rdf:resource="#OrgW3cDomHtmlLibrary"/>
		<rdfs:subClassOf rdf:resource="#OrgW3cDomLsLibrary"/>
		<rdfs:subClassOf rdf:resource="#OrgW3cDomTraversalLibrary"/>
		<rdfs:subClassOf rdf:resource="#OrgW3cDomRangesLibrary"/>
		<rdfs:subClassOf rdf:resource="#OrgW3cDomXpathLibrary"/>
		<rdfs:subClassOf rdf:resource="#OrgOmgCORBA_2_3Library"/>
		<rdfs:subClassOf rdf:resource="#OrgOmgCORBA_2_3PortableLibrary"/>
		<rdfs:subClassOf rdf:resource="#OrgOmgCORBALibrary"/>
		<rdfs:subClassOf rdf:resource="#OrgOmgCORBAPortableLibrary"/>
		<rdfs:subClassOf rdf:resource="#OrgOmgCORBADynAnyPackageLibrary"/>
		<rdfs:subClassOf rdf:resource="#OrgOmgCORBAORBPackageLibrary"/>
		<rdfs:subClassOf rdf:resource="#OrgOmgCORBATypeCodePackageLibrary"/>
		<rdfs:subClassOf rdf:resource="#OrgOmgCosNamingLibrary"/>
		<rdfs:subClassOf rdf:resource="#OrgOmgCosNamingNamingContextExtPackageLibrary"/>
		<rdfs:subClassOf rdf:resource="#OrgOmgCosNamingNamingContextPackageLibrary"/>
		<rdfs:subClassOf rdf:resource="#OrgOmgPortableServerLibrary"/>
		<rdfs:subClassOf rdf:resource="#OrgOmgPortableServerCurrentPackageLibrary"/>
		<rdfs:subClassOf rdf:resource="#OrgOmgPortableServerPOAManagerPackageLibrary"/>
		<rdfs:subClassOf rdf:resource="#OrgOmgPortableServerPOAPackageLibrary"/>
		<rdfs:subClassOf rdf:resource="#OrgOmgPortableServerServantLocatorPackageLibrary"/>
		<rdfs:subClassOf rdf:resource="#OrgOmgPortableServerPortableLibrary"/>
		<rdfs:subClassOf rdf:resource="#OrgOmgDynamicLibrary"/>
		<rdfs:subClassOf rdf:resource="#OrgOmgDynamicAnyLibrary"/>
		<rdfs:subClassOf rdf:resource="#OrgOmgDynamicAnyDynAnyFactoryPackageLibrary"/>
		<rdfs:subClassOf rdf:resource="#OrgOmgDynamicAnyDynAnyPackageLibrary"/>
		<rdfs:subClassOf rdf:resource="#OrgOmgIOPLibrary"/>
		<rdfs:subClassOf rdf:resource="#OrgOmgIOPCodecFactoryPackageLibrary"/>
		<rdfs:subClassOf rdf:resource="#OrgOmgIOPCodecPackageLibrary"/>
		<rdfs:subClassOf rdf:resource="#OrgOmgMessagingLibrary"/>
		<rdfs:subClassOf rdf:resource="#OrgOmgPortableInterceptorLibrary"/>
		<rdfs:subClassOf rdf:resource="#OrgOmgPortableInterceptorORBInitInfoPackageLibrary"/>
		<rdfs:subClassOf rdf:resource="#OrgOmgSendingContextLibrary"/>
		<rdfs:subClassOf rdf:resource="#OrgOmgStubJavaRmiLibrary"/>
		<rdfs:subClassOf rdf:resource="#OrgOmgStubJavaxManagementRemoteRmiLibrary"/>
		<rdfs:subClassOf rdf:resource="#OrgXmlSaxLibrary"/>
		<rdfs:subClassOf rdf:resource="#OrgXmlSaxExtLibrary"/>
		<rdfs:subClassOf rdf:resource="#OrgXmlSaxHelpersLibrary"/>
		<rdfs:subClassOf rdf:resource="#OrgIetfJgssLibrary"/>
		<rdfs:comment xml:lang="en">JavaLibrary implementing the entire API for j2se-1_6</rdfs:comment>
	</owl:Class>
	<owl:Class rdf:about="#J2se-1_6">
		<rdfs:subClassOf rdf:resource="&java;JRE"/>
		<rdfs:subClassOf>
			<owl:Restriction>
				<owl:onProperty rdf:resource="&java;providesBuiltinJavaLibrary"/>
				<owl:someValuesFrom rdf:resource="#J2se-1_6ClassLibrary"/>
			</owl:Restriction>
		</rdfs:subClassOf>
		<rdfs:comment xml:lang="en">j2se-1_6 Java Runtime Environment</rdfs:comment>
	</owl:Class>
	<owl:Class rdf:about="#JavaAppletLibrary">
		<rdfs:subClassOf rdf:resource="&j2se-1_5;JavaAppletLibrary"/>
		<rdfs:seeAlso rdf:resource="#JavaxAccessibilityLibrary"/>
		<rdfs:seeAlso rdf:resource="#JavaUtilLibrary"/>
		<rdfs:seeAlso rdf:resource="#JavaLangLibrary"/>
		<rdfs:seeAlso rdf:resource="#JavaIoLibrary"/>
		<rdfs:seeAlso rdf:resource="#JavaAwtLibrary"/>
		<rdfs:seeAlso rdf:resource="#JavaNetLibrary"/>
		<rdfs:comment xml:lang="en">JavaLibrary implementing the java.applet package for j2se-1_6</rdfs:comment>
	</owl:Class>
	<owl:Class rdf:about="#JavaAwtLibrary">
		<rdfs:subClassOf rdf:resource="&j2se-1_5;JavaAwtLibrary"/>
		<rdfs:seeAlso rdf:resource="#JavaUtilLibrary"/>
		<rdfs:seeAlso rdf:resource="#JavaLangLibrary"/>
		<rdfs:seeAlso rdf:resource="#JavaAwtEventLibrary"/>
		<rdfs:seeAlso rdf:resource="#JavaAwtImageLibrary"/>
		<rdfs:seeAlso rdf:resource="#JavaAwtPeerLibrary"/>
		<rdfs:seeAlso rdf:resource="#JavaxSwingTextLibrary"/>
		<rdfs:seeAlso rdf:resource="#JavaAwtImageRenderableLibrary"/>
		<rdfs:seeAlso rdf:resource="#JavaxAccessibilityLibrary"/>
		<rdfs:seeAlso rdf:resource="#JavaIoLibrary"/>
		<rdfs:seeAlso rdf:resource="#JavaAwtImLibrary"/>
		<rdfs:seeAlso rdf:resource="#JavaNetLibrary"/>
		<rdfs:seeAlso rdf:resource="#JavaAwtFontLibrary"/>
		<rdfs:seeAlso rdf:resource="#JavaBeansLibrary"/>
		<rdfs:seeAlso rdf:resource="#JavaSecurityLibrary"/>
		<rdfs:seeAlso rdf:resource="#JavaTextLibrary"/>
		<rdfs:seeAlso rdf:resource="#JavaAwtGeomLibrary"/>
		<rdfs:seeAlso rdf:resource="#JavaAwtDndLibrary"/>
		<rdfs:seeAlso rdf:resource="#JavaAwtDatatransferLibrary"/>
		<rdfs:seeAlso rdf:resource="#JavaAwtDndPeerLibrary"/>
		<rdfs:seeAlso rdf:resource="#JavaAwtColorLibrary"/>
		<rdfs:comment xml:lang="en">JavaLibrary implementing the java.awt package for j2se-1_6</rdfs:comment>
	</owl:Class>
	<owl:Class rdf:about="#JavaAwtEventLibrary">
		<rdfs:subClassOf rdf:resource="&j2se-1_5;JavaAwtEventLibrary"/>
		<rdfs:seeAlso rdf:resource="#JavaUtilLibrary"/>
		<rdfs:seeAlso rdf:resource="#JavaLangLibrary"/>
		<rdfs:seeAlso rdf:resource="#JavaAwtFontLibrary"/>
		<rdfs:seeAlso rdf:resource="#JavaAwtLibrary"/>
		<rdfs:seeAlso rdf:resource="#JavaTextLibrary"/>
		<rdfs:comment xml:lang="en">JavaLibrary implementing the java.awt.event package for j2se-1_6</rdfs:comment>
	</owl:Class>
	<owl:Class rdf:about="#JavaAwtColorLibrary">
		<owl:equivalentClass rdf:resource="&j2se-1_5;JavaAwtColorLibrary"/>
		<rdfs:subClassOf rdf:resource="&java;JavaLibrary"/>
		<rdfs:seeAlso rdf:resource="#JavaLangLibrary"/>
		<rdfs:seeAlso rdf:resource="#JavaIoLibrary"/>
		<rdfs:comment xml:lang="en">JavaLibrary implementing the java.awt.color package for j2se-1_6</rdfs:comment>
	</owl:Class>
	<owl:Class rdf:about="#JavaAwtDatatransferLibrary">
		<owl:equivalentClass rdf:resource="&j2se-1_5;JavaAwtDatatransferLibrary"/>
		<rdfs:subClassOf rdf:resource="&java;JavaLibrary"/>
		<rdfs:seeAlso rdf:resource="#JavaUtilLibrary"/>
		<rdfs:seeAlso rdf:resource="#JavaLangLibrary"/>
		<rdfs:seeAlso rdf:resource="#JavaIoLibrary"/>
		<rdfs:comment xml:lang="en">JavaLibrary implementing the java.awt.datatransfer package for j2se-1_6</rdfs:comment>
	</owl:Class>
	<owl:Class rdf:about="#JavaAwtDndLibrary">
		<owl:equivalentClass rdf:resource="&j2se-1_5;JavaAwtDndLibrary"/>
		<rdfs:subClassOf rdf:resource="&java;JavaLibrary"/>
		<rdfs:seeAlso rdf:resource="#JavaUtilLibrary"/>
		<rdfs:seeAlso rdf:resource="#JavaLangLibrary"/>
		<rdfs:seeAlso rdf:resource="#JavaIoLibrary"/>
		<rdfs:seeAlso rdf:resource="#JavaAwtLibrary"/>
		<rdfs:seeAlso rdf:resource="#JavaAwtPeerLibrary"/>
		<rdfs:seeAlso rdf:resource="#JavaAwtEventLibrary"/>
		<rdfs:seeAlso rdf:resource="#JavaAwtDatatransferLibrary"/>
		<rdfs:seeAlso rdf:resource="#JavaAwtDndPeerLibrary"/>
		<rdfs:comment xml:lang="en">JavaLibrary implementing the java.awt.dnd package for j2se-1_6</rdfs:comment>
	</owl:Class>
	<owl:Class rdf:about="#JavaAwtDndPeerLibrary">
		<owl:equivalentClass rdf:resource="&j2se-1_5;JavaAwtDndPeerLibrary"/>
		<rdfs:subClassOf rdf:resource="&java;JavaLibrary"/>
		<rdfs:seeAlso rdf:resource="#JavaAwtLibrary"/>
		<rdfs:seeAlso rdf:resource="#JavaAwtDatatransferLibrary"/>
		<rdfs:seeAlso rdf:resource="#JavaAwtDndLibrary"/>
		<rdfs:comment xml:lang="en">JavaLibrary implementing the java.awt.dnd.peer package for j2se-1_6</rdfs:comment>
	</owl:Class>
	<owl:Class rdf:about="#JavaAwtFontLibrary">
		<rdfs:subClassOf rdf:resource="&j2se-1_5;JavaAwtFontLibrary"/>
		<rdfs:seeAlso rdf:resource="#JavaUtilLibrary"/>
		<rdfs:seeAlso rdf:resource="#JavaLangLibrary"/>
		<rdfs:seeAlso rdf:resource="#JavaIoLibrary"/>
		<rdfs:seeAlso rdf:resource="#JavaAwtLibrary"/>
		<rdfs:seeAlso rdf:resource="#JavaTextLibrary"/>
		<rdfs:seeAlso rdf:resource="#JavaAwtGeomLibrary"/>
		<rdfs:comment xml:lang="en">JavaLibrary implementing the java.awt.font package for j2se-1_6</rdfs:comment>
	</owl:Class>
	<owl:Class rdf:about="#JavaAwtGeomLibrary">
		<rdfs:subClassOf rdf:resource="&java;JavaLibrary"/>
		<rdfs:seeAlso rdf:resource="#JavaAwtLibrary"/>
		<rdfs:seeAlso rdf:resource="#JavaLangLibrary"/>
		<rdfs:seeAlso rdf:resource="#JavaIoLibrary"/>
		<rdfs:comment xml:lang="en">JavaLibrary implementing the java.awt.geom package for j2se-1_6</rdfs:comment>
	</owl:Class>
	<owl:Class rdf:about="#JavaAwtImLibrary">
		<owl:equivalentClass rdf:resource="&j2se-1_5;JavaAwtImLibrary"/>
		<rdfs:subClassOf rdf:resource="&java;JavaLibrary"/>
		<rdfs:seeAlso rdf:resource="#JavaAwtFontLibrary"/>
		<rdfs:seeAlso rdf:resource="#JavaAwtLibrary"/>
		<rdfs:seeAlso rdf:resource="#JavaUtilLibrary"/>
		<rdfs:seeAlso rdf:resource="#JavaTextLibrary"/>
		<rdfs:seeAlso rdf:resource="#JavaLangLibrary"/>
		<rdfs:comment xml:lang="en">JavaLibrary implementing the java.awt.im package for j2se-1_6</rdfs:comment>
	</owl:Class>
	<owl:Class rdf:about="#JavaAwtImSpiLibrary">
		<owl:equivalentClass rdf:resource="&j2se-1_5;JavaAwtImSpiLibrary"/>
		<rdfs:subClassOf rdf:resource="&java;JavaLibrary"/>
		<rdfs:seeAlso rdf:resource="#JavaAwtFontLibrary"/>
		<rdfs:seeAlso rdf:resource="#JavaAwtLibrary"/>
		<rdfs:seeAlso rdf:resource="#JavaAwtImLibrary"/>
		<rdfs:seeAlso rdf:resource="#JavaxSwingLibrary"/>
		<rdfs:seeAlso rdf:resource="#JavaUtilLibrary"/>
		<rdfs:seeAlso rdf:resource="#JavaTextLibrary"/>
		<rdfs:seeAlso rdf:resource="#JavaLangLibrary"/>
		<rdfs:comment xml:lang="en">JavaLibrary implementing the java.awt.im.spi package for j2se-1_6</rdfs:comment>
	</owl:Class>
	<owl:Class rdf:about="#JavaAwtImageLibrary">
		<rdfs:subClassOf rdf:resource="&j2se-1_5;JavaAwtImageLibrary"/>
		<rdfs:seeAlso rdf:resource="#JavaUtilLibrary"/>
		<rdfs:seeAlso rdf:resource="#JavaLangLibrary"/>
		<rdfs:seeAlso rdf:resource="#JavaAwtLibrary"/>
		<rdfs:seeAlso rdf:resource="#JavaAwtColorLibrary"/>
		<rdfs:seeAlso rdf:resource="#JavaMathLibrary"/>
		<rdfs:seeAlso rdf:resource="#JavaAwtGeomLibrary"/>
		<rdfs:comment xml:lang="en">JavaLibrary implementing the java.awt.image package for j2se-1_6</rdfs:comment>
	</owl:Class>
	<owl:Class rdf:about="#JavaAwtImageRenderableLibrary">
		<owl:equivalentClass rdf:resource="&j2se-1_5;JavaAwtImageRenderableLibrary"/>
		<rdfs:subClassOf rdf:resource="&java;JavaLibrary"/>
		<rdfs:seeAlso rdf:resource="#JavaUtilLibrary"/>
		<rdfs:seeAlso rdf:resource="#JavaLangLibrary"/>
		<rdfs:seeAlso rdf:resource="#JavaIoLibrary"/>
		<rdfs:seeAlso rdf:resource="#JavaAwtLibrary"/>
		<rdfs:seeAlso rdf:resource="#JavaAwtImageLibrary"/>
		<rdfs:seeAlso rdf:resource="#JavaAwtGeomLibrary"/>
		<rdfs:comment xml:lang="en">JavaLibrary implementing the java.awt.image.renderable package for j2se-1_6</rdfs:comment>
	</owl:Class>
	<owl:Class rdf:about="#JavaAwtPeerLibrary">
		<rdfs:subClassOf rdf:resource="&java;JavaLibrary"/>
		<rdfs:seeAlso rdf:resource="#JavaLangLibrary"/>
		<rdfs:seeAlso rdf:resource="#JavaIoLibrary"/>
		<rdfs:seeAlso rdf:resource="#JavaAwtImLibrary"/>
		<rdfs:seeAlso rdf:resource="#JavaAwtLibrary"/>
		<rdfs:seeAlso rdf:resource="#JavaAwtImageLibrary"/>
		<rdfs:seeAlso rdf:resource="#JavaNetLibrary"/>
		<rdfs:seeAlso rdf:resource="#JavaAwtEventLibrary"/>
		<rdfs:comment xml:lang="en">JavaLibrary implementing the java.awt.peer package for j2se-1_6</rdfs:comment>
	</owl:Class>
	<owl:Class rdf:about="#JavaAwtPrintLibrary">
		<rdfs:subClassOf rdf:resource="&j2se-1_5;JavaAwtPrintLibrary"/>
		<rdfs:seeAlso rdf:resource="#JavaAwtLibrary"/>
		<rdfs:seeAlso rdf:resource="#JavaxPrintAttributeLibrary"/>
		<rdfs:seeAlso rdf:resource="#JavaxPrintLibrary"/>
		<rdfs:seeAlso rdf:resource="#JavaLangLibrary"/>
		<rdfs:seeAlso rdf:resource="#JavaIoLibrary"/>
		<rdfs:comment xml:lang="en">JavaLibrary implementing the java.awt.print package for j2se-1_6</rdfs:comment>
	</owl:Class>
	<owl:Class rdf:about="#JavaLangLibrary">
		<rdfs:subClassOf rdf:resource="&j2se-1_5;JavaLangLibrary"/>
		<rdfs:seeAlso rdf:resource="#JavaLangReflectLibrary"/>
		<rdfs:seeAlso rdf:resource="#JavaNioLibrary"/>
		<rdfs:seeAlso rdf:resource="#JavaUtilLibrary"/>
		<rdfs:seeAlso rdf:resource="#JavaSecurityLibrary"/>
		<rdfs:seeAlso rdf:resource="#JavaIoLibrary"/>
		<rdfs:seeAlso rdf:resource="#JavaNioCharsetLibrary"/>
		<rdfs:seeAlso rdf:resource="#JavaNetLibrary"/>
		<rdfs:seeAlso rdf:resource="#JavaLangAnnotationLibrary"/>
		<rdfs:seeAlso rdf:resource="#JavaNioChannelsLibrary"/>
		<rdfs:comment xml:lang="en">JavaLibrary implementing the java.lang package for j2se-1_6</rdfs:comment>
	</owl:Class>
	<owl:Class rdf:about="#JavaLangAnnotationLibrary">
		<rdfs:subClassOf rdf:resource="&j2se-1_5;JavaLangAnnotationLibrary"/>
		<rdfs:seeAlso rdf:resource="#JavaLangReflectLibrary"/>
		<rdfs:seeAlso rdf:resource="#JavaLangLibrary"/>
		<rdfs:comment xml:lang="en">JavaLibrary implementing the java.lang.annotation package for j2se-1_6</rdfs:comment>
	</owl:Class>
	<owl:Class rdf:about="#JavaLangReflectLibrary">
		<owl:equivalentClass rdf:resource="&j2se-1_5;JavaLangReflectLibrary"/>
		<rdfs:subClassOf rdf:resource="&java;JavaLibrary"/>
		<rdfs:seeAlso rdf:resource="#JavaLangAnnotationLibrary"/>
		<rdfs:seeAlso rdf:resource="#JavaSecurityLibrary"/>
		<rdfs:seeAlso rdf:resource="#JavaLangLibrary"/>
		<rdfs:seeAlso rdf:resource="#JavaIoLibrary"/>
		<rdfs:comment xml:lang="en">JavaLibrary implementing the java.lang.reflect package for j2se-1_6</rdfs:comment>
	</owl:Class>
	<owl:Class rdf:about="#JavaLangInstrumentLibrary">
		<rdfs:subClassOf rdf:resource="&j2se-1_5;JavaLangInstrumentLibrary"/>
		<rdfs:seeAlso rdf:resource="#JavaUtilJarLibrary"/>
		<rdfs:seeAlso rdf:resource="#JavaSecurityLibrary"/>
		<rdfs:seeAlso rdf:resource="#JavaLangLibrary"/>
		<rdfs:comment xml:lang="en">JavaLibrary implementing the java.lang.instrument package for j2se-1_6</rdfs:comment>
	</owl:Class>
	<owl:Class rdf:about="#JavaLangManagementLibrary">
		<rdfs:subClassOf rdf:resource="&j2se-1_5;JavaLangManagementLibrary"/>
		<rdfs:seeAlso rdf:resource="#JavaxManagementLibrary"/>
		<rdfs:seeAlso rdf:resource="#JavaUtilLibrary"/>
		<rdfs:seeAlso rdf:resource="#JavaSecurityLibrary"/>
		<rdfs:seeAlso rdf:resource="#JavaLangLibrary"/>
		<rdfs:seeAlso rdf:resource="#JavaxManagementOpenmbeanLibrary"/>
		<rdfs:comment xml:lang="en">JavaLibrary implementing the java.lang.management package for j2se-1_6</rdfs:comment>
	</owl:Class>
	<owl:Class rdf:about="#JavaLangRefLibrary">
		<owl:equivalentClass rdf:resource="&j2se-1_5;JavaLangRefLibrary"/>
		<rdfs:subClassOf rdf:resource="&java;JavaLibrary"/>
		<rdfs:seeAlso rdf:resource="#JavaLangLibrary"/>
		<rdfs:comment xml:lang="en">JavaLibrary implementing the java.lang.ref package for j2se-1_6</rdfs:comment>
	</owl:Class>
	<owl:Class rdf:about="#JavaIoLibrary">
		<rdfs:subClassOf rdf:resource="&j2se-1_5;JavaIoLibrary"/>
		<rdfs:seeAlso rdf:resource="#JavaNioLibrary"/>
		<rdfs:seeAlso rdf:resource="#JavaNioChannelsLibrary"/>
		<rdfs:seeAlso rdf:resource="#JavaUtilLibrary"/>
		<rdfs:seeAlso rdf:resource="#JavaSecurityLibrary"/>
		<rdfs:seeAlso rdf:resource="#JavaLangLibrary"/>
		<rdfs:seeAlso rdf:resource="#JavaNioCharsetLibrary"/>
		<rdfs:seeAlso rdf:resource="#JavaNetLibrary"/>
		<rdfs:comment xml:lang="en">JavaLibrary implementing the java.io package for j2se-1_6</rdfs:comment>
	</owl:Class>
	<owl:Class rdf:about="#JavaUtilLibrary">
		<rdfs:subClassOf rdf:resource="&j2se-1_5;JavaUtilLibrary"/>
		<rdfs:seeAlso rdf:resource="#JavaSecurityLibrary"/>
		<rdfs:seeAlso rdf:resource="#JavaLangLibrary"/>
		<rdfs:seeAlso rdf:resource="#JavaIoLibrary"/>
		<rdfs:seeAlso rdf:resource="#JavaMathLibrary"/>
		<rdfs:seeAlso rdf:resource="#JavaUtilRegexLibrary"/>
		<rdfs:seeAlso rdf:resource="#JavaNioChannelsLibrary"/>
		<rdfs:comment xml:lang="en">JavaLibrary implementing the java.util package for j2se-1_6</rdfs:comment>
	</owl:Class>
	<owl:Class rdf:about="#JavaUtilSpiLibrary">
		<rdfs:subClassOf rdf:resource="&java;JavaLibrary"/>
		<rdfs:seeAlso rdf:resource="#JavaUtilLibrary"/>
		<rdfs:seeAlso rdf:resource="#JavaLangLibrary"/>
		<rdfs:comment xml:lang="en">JavaLibrary implementing the java.util.spi package for j2se-1_6</rdfs:comment>
	</owl:Class>
	<owl:Class rdf:about="#JavaUtilConcurrentLibrary">
		<rdfs:subClassOf rdf:resource="&java;JavaLibrary"/>
		<rdfs:seeAlso rdf:resource="#JavaUtilLibrary"/>
		<rdfs:seeAlso rdf:resource="#JavaSecurityLibrary"/>
		<rdfs:seeAlso rdf:resource="#JavaLangLibrary"/>
		<rdfs:seeAlso rdf:resource="#JavaIoLibrary"/>
		<rdfs:comment xml:lang="en">JavaLibrary implementing the java.util.concurrent package for j2se-1_6</rdfs:comment>
	</owl:Class>
	<owl:Class rdf:about="#JavaUtilConcurrentAtomicLibrary">
		<rdfs:subClassOf rdf:resource="&j2se-1_5;JavaUtilConcurrentAtomicLibrary"/>
		<rdfs:seeAlso rdf:resource="#JavaLangLibrary"/>
		<rdfs:seeAlso rdf:resource="#JavaIoLibrary"/>
		<rdfs:comment xml:lang="en">JavaLibrary implementing the java.util.concurrent.atomic package for j2se-1_6</rdfs:comment>
	</owl:Class>
	<owl:Class rdf:about="#JavaUtilConcurrentLocksLibrary">
		<rdfs:subClassOf rdf:resource="&j2se-1_5;JavaUtilConcurrentLocksLibrary"/>
		<rdfs:seeAlso rdf:resource="#JavaUtilConcurrentLibrary"/>
		<rdfs:seeAlso rdf:resource="#JavaUtilLibrary"/>
		<rdfs:seeAlso rdf:resource="#JavaLangLibrary"/>
		<rdfs:seeAlso rdf:resource="#JavaIoLibrary"/>
		<rdfs:comment xml:lang="en">JavaLibrary implementing the java.util.concurrent.locks package for j2se-1_6</rdfs:comment>
	</owl:Class>
	<owl:Class rdf:about="#JavaUtilJarLibrary">
		<owl:equivalentClass rdf:resource="&j2se-1_5;JavaUtilJarLibrary"/>
		<rdfs:subClassOf rdf:resource="&java;JavaLibrary"/>
		<rdfs:seeAlso rdf:resource="#JavaUtilLibrary"/>
		<rdfs:seeAlso rdf:resource="#JavaLangLibrary"/>
		<rdfs:seeAlso rdf:resource="#JavaIoLibrary"/>
		<rdfs:seeAlso rdf:resource="#JavaBeansLibrary"/>
		<rdfs:seeAlso rdf:resource="#JavaUtilZipLibrary"/>
		<rdfs:comment xml:lang="en">JavaLibrary implementing the java.util.jar package for j2se-1_6</rdfs:comment>
	</owl:Class>
	<owl:Class rdf:about="#JavaUtilZipLibrary">
		<rdfs:subClassOf rdf:resource="&j2se-1_5;JavaUtilZipLibrary"/>
		<rdfs:seeAlso rdf:resource="#JavaUtilLibrary"/>
		<rdfs:seeAlso rdf:resource="#JavaLangLibrary"/>
		<rdfs:seeAlso rdf:resource="#JavaIoLibrary"/>
		<rdfs:comment xml:lang="en">JavaLibrary implementing the java.util.zip package for j2se-1_6</rdfs:comment>
	</owl:Class>
	<owl:Class rdf:about="#JavaUtilLoggingLibrary">
		<rdfs:subClassOf rdf:resource="&j2se-1_5;JavaUtilLoggingLibrary"/>
		<rdfs:seeAlso rdf:resource="#JavaUtilLibrary"/>
		<rdfs:seeAlso rdf:resource="#JavaSecurityLibrary"/>
		<rdfs:seeAlso rdf:resource="#JavaLangLibrary"/>
		<rdfs:seeAlso rdf:resource="#JavaIoLibrary"/>
		<rdfs:seeAlso rdf:resource="#JavaBeansLibrary"/>
		<rdfs:comment xml:lang="en">JavaLibrary implementing the java.util.logging package for j2se-1_6</rdfs:comment>
	</owl:Class>
	<owl:Class rdf:about="#JavaUtilPrefsLibrary">
		<owl:equivalentClass rdf:resource="&j2se-1_5;JavaUtilPrefsLibrary"/>
		<rdfs:subClassOf rdf:resource="&java;JavaLibrary"/>
		<rdfs:seeAlso rdf:resource="#JavaUtilLibrary"/>
		<rdfs:seeAlso rdf:resource="#JavaLangLibrary"/>
		<rdfs:seeAlso rdf:resource="#JavaIoLibrary"/>
		<rdfs:comment xml:lang="en">JavaLibrary implementing the java.util.prefs package for j2se-1_6</rdfs:comment>
	</owl:Class>
	<owl:Class rdf:about="#JavaUtilRegexLibrary">
		<owl:equivalentClass rdf:resource="&j2se-1_5;JavaUtilRegexLibrary"/>
		<rdfs:subClassOf rdf:resource="&java;JavaLibrary"/>
		<rdfs:seeAlso rdf:resource="#JavaLangLibrary"/>
		<rdfs:seeAlso rdf:resource="#JavaIoLibrary"/>
		<rdfs:comment xml:lang="en">JavaLibrary implementing the java.util.regex package for j2se-1_6</rdfs:comment>
	</owl:Class>
	<owl:Class rdf:about="#JavaBeansLibrary">
		<rdfs:subClassOf rdf:resource="&j2se-1_5;JavaBeansLibrary"/>
		<rdfs:seeAlso rdf:resource="#JavaLangAnnotationLibrary"/>
		<rdfs:seeAlso rdf:resource="#JavaLangReflectLibrary"/>
		<rdfs:seeAlso rdf:resource="#JavaBeansBeancontextLibrary"/>
		<rdfs:seeAlso rdf:resource="#JavaAppletLibrary"/>
		<rdfs:seeAlso rdf:resource="#JavaUtilLibrary"/>
		<rdfs:seeAlso rdf:resource="#JavaLangLibrary"/>
		<rdfs:seeAlso rdf:resource="#JavaIoLibrary"/>
		<rdfs:seeAlso rdf:resource="#JavaAwtLibrary"/>
		<rdfs:comment xml:lang="en">JavaLibrary implementing the java.beans package for j2se-1_6</rdfs:comment>
	</owl:Class>
	<owl:Class rdf:about="#JavaBeansBeancontextLibrary">
		<owl:equivalentClass rdf:resource="&j2se-1_5;JavaBeansBeancontextLibrary"/>
		<rdfs:subClassOf rdf:resource="&java;JavaLibrary"/>
		<rdfs:seeAlso rdf:resource="#JavaUtilLibrary"/>
		<rdfs:seeAlso rdf:resource="#JavaLangLibrary"/>
		<rdfs:seeAlso rdf:resource="#JavaIoLibrary"/>
		<rdfs:seeAlso rdf:resource="#JavaAwtLibrary"/>
		<rdfs:seeAlso rdf:resource="#JavaNetLibrary"/>
		<rdfs:seeAlso rdf:resource="#JavaBeansLibrary"/>
		<rdfs:comment xml:lang="en">JavaLibrary implementing the java.beans.beancontext package for j2se-1_6</rdfs:comment>
	</owl:Class>
	<owl:Class rdf:about="#JavaSecurityLibrary">
		<rdfs:subClassOf rdf:resource="&j2se-1_5;JavaSecurityLibrary"/>
		<rdfs:seeAlso rdf:resource="#JavaxSecurityAuthCallbackLibrary"/>
		<rdfs:seeAlso rdf:resource="#JavaxSecurityAuthLibrary"/>
		<rdfs:seeAlso rdf:resource="#JavaNioLibrary"/>
		<rdfs:seeAlso rdf:resource="#JavaSecurityCertLibrary"/>
		<rdfs:seeAlso rdf:resource="#JavaUtilLibrary"/>
		<rdfs:seeAlso rdf:resource="#JavaLangLibrary"/>
		<rdfs:seeAlso rdf:resource="#JavaIoLibrary"/>
		<rdfs:seeAlso rdf:resource="#JavaNetLibrary"/>
		<rdfs:seeAlso rdf:resource="#JavaxCryptoLibrary"/>
		<rdfs:seeAlso rdf:resource="#JavaxSecurityAuthLoginLibrary"/>
		<rdfs:seeAlso rdf:resource="#JavaSecuritySpecLibrary"/>
		<rdfs:comment xml:lang="en">JavaLibrary implementing the java.security package for j2se-1_6</rdfs:comment>
	</owl:Class>
	<owl:Class rdf:about="#JavaSecurityAclLibrary">
		<owl:equivalentClass rdf:resource="&j2se-1_5;JavaSecurityAclLibrary"/>
		<rdfs:subClassOf rdf:resource="&java;JavaLibrary"/>
		<rdfs:seeAlso rdf:resource="#JavaUtilLibrary"/>
		<rdfs:seeAlso rdf:resource="#JavaSecurityLibrary"/>
		<rdfs:seeAlso rdf:resource="#JavaLangLibrary"/>
		<rdfs:comment xml:lang="en">JavaLibrary implementing the java.security.acl package for j2se-1_6</rdfs:comment>
	</owl:Class>
	<owl:Class rdf:about="#JavaSecurityCertLibrary">
		<owl:equivalentClass rdf:resource="&j2se-1_5;JavaSecurityCertLibrary"/>
		<rdfs:subClassOf rdf:resource="&java;JavaLibrary"/>
		<rdfs:seeAlso rdf:resource="#JavaUtilLibrary"/>
		<rdfs:seeAlso rdf:resource="#JavaSecurityLibrary"/>
		<rdfs:seeAlso rdf:resource="#JavaLangLibrary"/>
		<rdfs:seeAlso rdf:resource="#JavaIoLibrary"/>
		<rdfs:seeAlso rdf:resource="#JavaMathLibrary"/>
		<rdfs:seeAlso rdf:resource="#JavaxSecurityAuthX500Library"/>
		<rdfs:comment xml:lang="en">JavaLibrary implementing the java.security.cert package for j2se-1_6</rdfs:comment>
	</owl:Class>
	<owl:Class rdf:about="#JavaSecurityInterfacesLibrary">
		<owl:equivalentClass rdf:resource="&j2se-1_5;JavaSecurityInterfacesLibrary"/>
		<rdfs:subClassOf rdf:resource="&java;JavaLibrary"/>
		<rdfs:seeAlso rdf:resource="#JavaMathLibrary"/>
		<rdfs:seeAlso rdf:resource="#JavaSecuritySpecLibrary"/>
		<rdfs:seeAlso rdf:resource="#JavaSecurityLibrary"/>
		<rdfs:comment xml:lang="en">JavaLibrary implementing the java.security.interfaces package for j2se-1_6</rdfs:comment>
	</owl:Class>
	<owl:Class rdf:about="#JavaSecuritySpecLibrary">
		<owl:equivalentClass rdf:resource="&j2se-1_5;JavaSecuritySpecLibrary"/>
		<rdfs:subClassOf rdf:resource="&java;JavaLibrary"/>
		<rdfs:seeAlso rdf:resource="#JavaMathLibrary"/>
		<rdfs:seeAlso rdf:resource="#JavaSecurityInterfacesLibrary"/>
		<rdfs:seeAlso rdf:resource="#JavaSecurityLibrary"/>
		<rdfs:seeAlso rdf:resource="#JavaLangLibrary"/>
		<rdfs:comment xml:lang="en">JavaLibrary implementing the java.security.spec package for j2se-1_6</rdfs:comment>
	</owl:Class>
	<owl:Class rdf:about="#JavaMathLibrary">
		<rdfs:subClassOf rdf:resource="&j2se-1_5;JavaMathLibrary"/>
		<rdfs:seeAlso rdf:resource="#JavaUtilLibrary"/>
		<rdfs:seeAlso rdf:resource="#JavaLangLibrary"/>
		<rdfs:seeAlso rdf:resource="#JavaIoLibrary"/>
		<rdfs:comment xml:lang="en">JavaLibrary implementing the java.math package for j2se-1_6</rdfs:comment>
	</owl:Class>
	<owl:Class rdf:about="#JavaNetLibrary">
		<rdfs:subClassOf rdf:resource="&j2se-1_5;JavaNetLibrary"/>
		<rdfs:seeAlso rdf:resource="#JavaUtilJarLibrary"/>
		<rdfs:seeAlso rdf:resource="#JavaUtilLibrary"/>
		<rdfs:seeAlso rdf:resource="#JavaSecurityLibrary"/>
		<rdfs:seeAlso rdf:resource="#JavaLangLibrary"/>
		<rdfs:seeAlso rdf:resource="#JavaIoLibrary"/>
		<rdfs:seeAlso rdf:resource="#JavaNioChannelsLibrary"/>
		<rdfs:comment xml:lang="en">JavaLibrary implementing the java.net package for j2se-1_6</rdfs:comment>
	</owl:Class>
	<owl:Class rdf:about="#JavaNioLibrary">
		<rdfs:subClassOf rdf:resource="&j2se-1_5;JavaNioLibrary"/>
		<rdfs:seeAlso rdf:resource="#JavaLangLibrary"/>
		<rdfs:comment xml:lang="en">JavaLibrary implementing the java.nio package for j2se-1_6</rdfs:comment>
	</owl:Class>
	<owl:Class rdf:about="#JavaNioChannelsLibrary">
		<owl:equivalentClass rdf:resource="&j2se-1_5;JavaNioChannelsLibrary"/>
		<rdfs:subClassOf rdf:resource="&java;JavaLibrary"/>
		<rdfs:seeAlso rdf:resource="#JavaNioLibrary"/>
		<rdfs:seeAlso rdf:resource="#JavaUtilLibrary"/>
		<rdfs:seeAlso rdf:resource="#JavaLangLibrary"/>
		<rdfs:seeAlso rdf:resource="#JavaIoLibrary"/>
		<rdfs:seeAlso rdf:resource="#JavaNioChannelsSpiLibrary"/>
		<rdfs:seeAlso rdf:resource="#JavaNioCharsetLibrary"/>
		<rdfs:seeAlso rdf:resource="#JavaNetLibrary"/>
		<rdfs:comment xml:lang="en">JavaLibrary implementing the java.nio.channels package for j2se-1_6</rdfs:comment>
	</owl:Class>
	<owl:Class rdf:about="#JavaNioChannelsSpiLibrary">
		<owl:equivalentClass rdf:resource="&j2se-1_5;JavaNioChannelsSpiLibrary"/>
		<rdfs:subClassOf rdf:resource="&java;JavaLibrary"/>
		<rdfs:seeAlso rdf:resource="#JavaNioChannelsLibrary"/>
		<rdfs:seeAlso rdf:resource="#JavaUtilLibrary"/>
		<rdfs:seeAlso rdf:resource="#JavaLangLibrary"/>
		<rdfs:comment xml:lang="en">JavaLibrary implementing the java.nio.channels.spi package for j2se-1_6</rdfs:comment>
	</owl:Class>
	<owl:Class rdf:about="#JavaNioCharsetLibrary">
		<owl:equivalentClass rdf:resource="&j2se-1_5;JavaNioCharsetLibrary"/>
		<rdfs:subClassOf rdf:resource="&java;JavaLibrary"/>
		<rdfs:seeAlso rdf:resource="#JavaNioLibrary"/>
		<rdfs:seeAlso rdf:resource="#JavaUtilLibrary"/>
		<rdfs:seeAlso rdf:resource="#JavaLangLibrary"/>
		<rdfs:seeAlso rdf:resource="#JavaIoLibrary"/>
		<rdfs:comment xml:lang="en">JavaLibrary implementing the java.nio.charset package for j2se-1_6</rdfs:comment>
	</owl:Class>
	<owl:Class rdf:about="#JavaNioCharsetSpiLibrary">
		<owl:equivalentClass rdf:resource="&j2se-1_5;JavaNioCharsetSpiLibrary"/>
		<rdfs:subClassOf rdf:resource="&java;JavaLibrary"/>
		<rdfs:seeAlso rdf:resource="#JavaUtilLibrary"/>
		<rdfs:seeAlso rdf:resource="#JavaNioCharsetLibrary"/>
		<rdfs:seeAlso rdf:resource="#JavaLangLibrary"/>
		<rdfs:comment xml:lang="en">JavaLibrary implementing the java.nio.charset.spi package for j2se-1_6</rdfs:comment>
	</owl:Class>
	<owl:Class rdf:about="#JavaRmiLibrary">
		<owl:equivalentClass rdf:resource="&j2se-1_5;JavaRmiLibrary"/>
		<rdfs:subClassOf rdf:resource="&java;JavaLibrary"/>
		<rdfs:seeAlso rdf:resource="#JavaLangLibrary"/>
		<rdfs:seeAlso rdf:resource="#JavaIoLibrary"/>
		<rdfs:comment xml:lang="en">JavaLibrary implementing the java.rmi package for j2se-1_6</rdfs:comment>
	</owl:Class>
	<owl:Class rdf:about="#JavaRmiActivationLibrary">
		<owl:equivalentClass rdf:resource="&j2se-1_5;JavaRmiActivationLibrary"/>
		<rdfs:subClassOf rdf:resource="&java;JavaLibrary"/>
		<rdfs:seeAlso rdf:resource="#JavaUtilLibrary"/>
		<rdfs:seeAlso rdf:resource="#JavaLangLibrary"/>
		<rdfs:seeAlso rdf:resource="#JavaRmiLibrary"/>
		<rdfs:seeAlso rdf:resource="#JavaIoLibrary"/>
		<rdfs:seeAlso rdf:resource="#JavaRmiServerLibrary"/>
		<rdfs:comment xml:lang="en">JavaLibrary implementing the java.rmi.activation package for j2se-1_6</rdfs:comment>
	</owl:Class>
	<owl:Class rdf:about="#JavaRmiServerLibrary">
		<rdfs:subClassOf rdf:resource="&j2se-1_5;JavaRmiServerLibrary"/>
		<rdfs:seeAlso rdf:resource="#JavaLangReflectLibrary"/>
		<rdfs:seeAlso rdf:resource="#JavaRmiLibrary"/>
		<rdfs:seeAlso rdf:resource="#JavaLangLibrary"/>
		<rdfs:seeAlso rdf:resource="#JavaIoLibrary"/>
		<rdfs:seeAlso rdf:resource="#JavaNetLibrary"/>
		<rdfs:comment xml:lang="en">JavaLibrary implementing the java.rmi.server package for j2se-1_6</rdfs:comment>
	</owl:Class>
	<owl:Class rdf:about="#JavaRmiDgcLibrary">
		<owl:equivalentClass rdf:resource="&j2se-1_5;JavaRmiDgcLibrary"/>
		<rdfs:subClassOf rdf:resource="&java;JavaLibrary"/>
		<rdfs:seeAlso rdf:resource="#JavaRmiLibrary"/>
		<rdfs:seeAlso rdf:resource="#JavaLangLibrary"/>
		<rdfs:seeAlso rdf:resource="#JavaIoLibrary"/>
		<rdfs:comment xml:lang="en">JavaLibrary implementing the java.rmi.dgc package for j2se-1_6</rdfs:comment>
	</owl:Class>
	<owl:Class rdf:about="#JavaRmiRegistryLibrary">
		<owl:equivalentClass rdf:resource="&j2se-1_5;JavaRmiRegistryLibrary"/>
		<rdfs:subClassOf rdf:resource="&java;JavaLibrary"/>
		<rdfs:seeAlso rdf:resource="#JavaLangLibrary"/>
		<rdfs:seeAlso rdf:resource="#JavaRmiLibrary"/>
		<rdfs:seeAlso rdf:resource="#JavaRmiServerLibrary"/>
		<rdfs:comment xml:lang="en">JavaLibrary implementing the java.rmi.registry package for j2se-1_6</rdfs:comment>
	</owl:Class>
	<owl:Class rdf:about="#JavaSqlLibrary">
		<rdfs:subClassOf rdf:resource="&j2se-1_5;JavaSqlLibrary"/>
		<rdfs:seeAlso rdf:resource="#JavaUtilLibrary"/>
		<rdfs:seeAlso rdf:resource="#JavaSecurityLibrary"/>
		<rdfs:seeAlso rdf:resource="#JavaLangLibrary"/>
		<rdfs:seeAlso rdf:resource="#JavaIoLibrary"/>
		<rdfs:seeAlso rdf:resource="#JavaMathLibrary"/>
		<rdfs:seeAlso rdf:resource="#JavaNetLibrary"/>
		<rdfs:seeAlso rdf:resource="#JavaxXmlTransformLibrary"/>
		<rdfs:comment xml:lang="en">JavaLibrary implementing the java.sql package for j2se-1_6</rdfs:comment>
	</owl:Class>
	<owl:Class rdf:about="#JavaTextLibrary">
		<rdfs:subClassOf rdf:resource="&java;JavaLibrary"/>
		<rdfs:seeAlso rdf:resource="#JavaUtilLibrary"/>
		<rdfs:seeAlso rdf:resource="#JavaLangLibrary"/>
		<rdfs:seeAlso rdf:resource="#JavaIoLibrary"/>
		<rdfs:seeAlso rdf:resource="#JavaMathLibrary"/>
		<rdfs:comment xml:lang="en">JavaLibrary implementing the java.text package for j2se-1_6</rdfs:comment>
	</owl:Class>
	<owl:Class rdf:about="#JavaTextSpiLibrary">
		<rdfs:subClassOf rdf:resource="&java;JavaLibrary"/>
		<rdfs:seeAlso rdf:resource="#JavaUtilSpiLibrary"/>
		<rdfs:seeAlso rdf:resource="#JavaUtilLibrary"/>
		<rdfs:seeAlso rdf:resource="#JavaTextLibrary"/>
		<rdfs:comment xml:lang="en">JavaLibrary implementing the java.text.spi package for j2se-1_6</rdfs:comment>
	</owl:Class>
	<owl:Class rdf:about="#JavaxAccessibilityLibrary">
		<rdfs:subClassOf rdf:resource="&j2se-1_5;JavaxAccessibilityLibrary"/>
		<rdfs:seeAlso rdf:resource="#JavaAwtEventLibrary"/>
		<rdfs:seeAlso rdf:resource="#JavaAwtDatatransferLibrary"/>
		<rdfs:seeAlso rdf:resource="#JavaxSwingTextLibrary"/>
		<rdfs:seeAlso rdf:resource="#JavaUtilLibrary"/>
		<rdfs:seeAlso rdf:resource="#JavaLangLibrary"/>
		<rdfs:seeAlso rdf:resource="#JavaIoLibrary"/>
		<rdfs:seeAlso rdf:resource="#JavaAwtLibrary"/>
		<rdfs:seeAlso rdf:resource="#JavaBeansLibrary"/>
		<rdfs:comment xml:lang="en">JavaLibrary implementing the javax.accessibility package for j2se-1_6</rdfs:comment>
	</owl:Class>
	<owl:Class rdf:about="#JavaxSecurityAuthLibrary">
		<owl:equivalentClass rdf:resource="&j2se-1_5;JavaxSecurityAuthLibrary"/>
		<rdfs:subClassOf rdf:resource="&java;JavaLibrary"/>
		<rdfs:seeAlso rdf:resource="#JavaUtilLibrary"/>
		<rdfs:seeAlso rdf:resource="#JavaSecurityLibrary"/>
		<rdfs:seeAlso rdf:resource="#JavaLangLibrary"/>
		<rdfs:seeAlso rdf:resource="#JavaIoLibrary"/>
		<rdfs:comment xml:lang="en">JavaLibrary implementing the javax.security.auth package for j2se-1_6</rdfs:comment>
	</owl:Class>
	<owl:Class rdf:about="#JavaxSecurityAuthLoginLibrary">
		<rdfs:subClassOf rdf:resource="&j2se-1_5;JavaxSecurityAuthLoginLibrary"/>
		<rdfs:seeAlso rdf:resource="#JavaxSecurityAuthCallbackLibrary"/>
		<rdfs:seeAlso rdf:resource="#JavaxSecurityAuthLibrary"/>
		<rdfs:seeAlso rdf:resource="#JavaUtilLibrary"/>
		<rdfs:seeAlso rdf:resource="#JavaSecurityLibrary"/>
		<rdfs:seeAlso rdf:resource="#JavaLangLibrary"/>
		<rdfs:comment xml:lang="en">JavaLibrary implementing the javax.security.auth.login package for j2se-1_6</rdfs:comment>
	</owl:Class>
	<owl:Class rdf:about="#JavaxSecurityAuthCallbackLibrary">
		<owl:equivalentClass rdf:resource="&j2se-1_5;JavaxSecurityAuthCallbackLibrary"/>
		<rdfs:subClassOf rdf:resource="&java;JavaLibrary"/>
		<rdfs:seeAlso rdf:resource="#JavaUtilLibrary"/>
		<rdfs:seeAlso rdf:resource="#JavaLangLibrary"/>
		<rdfs:seeAlso rdf:resource="#JavaIoLibrary"/>
		<rdfs:comment xml:lang="en">JavaLibrary implementing the javax.security.auth.callback package for j2se-1_6</rdfs:comment>
	</owl:Class>
	<owl:Class rdf:about="#JavaxSecurityAuthKerberosLibrary">
		<owl:equivalentClass rdf:resource="&j2se-1_5;JavaxSecurityAuthKerberosLibrary"/>
		<rdfs:subClassOf rdf:resource="&java;JavaLibrary"/>
		<rdfs:seeAlso rdf:resource="#JavaxCryptoLibrary"/>
		<rdfs:seeAlso rdf:resource="#JavaxSecurityAuthLibrary"/>
		<rdfs:seeAlso rdf:resource="#JavaUtilLibrary"/>
		<rdfs:seeAlso rdf:resource="#JavaSecurityLibrary"/>
		<rdfs:seeAlso rdf:resource="#JavaLangLibrary"/>
		<rdfs:seeAlso rdf:resource="#JavaIoLibrary"/>
		<rdfs:comment xml:lang="en">JavaLibrary implementing the javax.security.auth.kerberos package for j2se-1_6</rdfs:comment>
	</owl:Class>
	<owl:Class rdf:about="#JavaxSecurityAuthSpiLibrary">
		<owl:equivalentClass rdf:resource="&j2se-1_5;JavaxSecurityAuthSpiLibrary"/>
		<rdfs:subClassOf rdf:resource="&java;JavaLibrary"/>
		<rdfs:seeAlso rdf:resource="#JavaxSecurityAuthCallbackLibrary"/>
		<rdfs:seeAlso rdf:resource="#JavaxSecurityAuthLibrary"/>
		<rdfs:seeAlso rdf:resource="#JavaUtilLibrary"/>
		<rdfs:comment xml:lang="en">JavaLibrary implementing the javax.security.auth.spi package for j2se-1_6</rdfs:comment>
	</owl:Class>
	<owl:Class rdf:about="#JavaxSecurityAuthX500Library">
		<rdfs:subClassOf rdf:resource="&j2se-1_5;JavaxSecurityAuthX500Library"/>
		<rdfs:seeAlso rdf:resource="#JavaxSecurityAuthLibrary"/>
		<rdfs:seeAlso rdf:resource="#JavaSecurityCertLibrary"/>
		<rdfs:seeAlso rdf:resource="#JavaUtilLibrary"/>
		<rdfs:seeAlso rdf:resource="#JavaSecurityLibrary"/>
		<rdfs:seeAlso rdf:resource="#JavaLangLibrary"/>
		<rdfs:seeAlso rdf:resource="#JavaIoLibrary"/>
		<rdfs:comment xml:lang="en">JavaLibrary implementing the javax.security.auth.x500 package for j2se-1_6</rdfs:comment>
	</owl:Class>
	<owl:Class rdf:about="#JavaxSecuritySaslLibrary">
		<rdfs:subClassOf rdf:resource="&j2se-1_5;JavaxSecuritySaslLibrary"/>
		<rdfs:seeAlso rdf:resource="#JavaxSecurityAuthCallbackLibrary"/>
		<rdfs:seeAlso rdf:resource="#JavaUtilLibrary"/>
		<rdfs:seeAlso rdf:resource="#JavaLangLibrary"/>
		<rdfs:seeAlso rdf:resource="#JavaIoLibrary"/>
		<rdfs:comment xml:lang="en">JavaLibrary implementing the javax.security.sasl package for j2se-1_6</rdfs:comment>
	</owl:Class>
	<owl:Class rdf:about="#JavaxActivationLibrary">
		<rdfs:subClassOf rdf:resource="&java;JavaLibrary"/>
		<rdfs:seeAlso rdf:resource="#JavaAwtDatatransferLibrary"/>
		<rdfs:seeAlso rdf:resource="#JavaUtilLibrary"/>
		<rdfs:seeAlso rdf:resource="#JavaLangLibrary"/>
		<rdfs:seeAlso rdf:resource="#JavaIoLibrary"/>
		<rdfs:seeAlso rdf:resource="#JavaNetLibrary"/>
		<rdfs:comment xml:lang="en">JavaLibrary implementing the javax.activation package for j2se-1_6</rdfs:comment>
	</owl:Class>
	<owl:Class rdf:about="#JavaxActivityLibrary">
		<owl:equivalentClass rdf:resource="&j2se-1_5;JavaxActivityLibrary"/>
		<rdfs:subClassOf rdf:resource="&java;JavaLibrary"/>
		<rdfs:seeAlso rdf:resource="#JavaLangLibrary"/>
		<rdfs:seeAlso rdf:resource="#JavaRmiLibrary"/>
		<rdfs:comment xml:lang="en">JavaLibrary implementing the javax.activity package for j2se-1_6</rdfs:comment>
	</owl:Class>
	<owl:Class rdf:about="#JavaxAnnotationLibrary">
		<rdfs:subClassOf rdf:resource="&java;JavaLibrary"/>
		<rdfs:seeAlso rdf:resource="#JavaLangAnnotationLibrary"/>
		<rdfs:seeAlso rdf:resource="#JavaLangLibrary"/>
		<rdfs:comment xml:lang="en">JavaLibrary implementing the javax.annotation package for j2se-1_6</rdfs:comment>
	</owl:Class>
	<owl:Class rdf:about="#JavaxAnnotationProcessingLibrary">
		<rdfs:subClassOf rdf:resource="&java;JavaLibrary"/>
		<rdfs:seeAlso rdf:resource="#JavaLangAnnotationLibrary"/>
		<rdfs:seeAlso rdf:resource="#JavaxLangModelUtilLibrary"/>
		<rdfs:seeAlso rdf:resource="#JavaxLangModelElementLibrary"/>
		<rdfs:seeAlso rdf:resource="#JavaUtilLibrary"/>
		<rdfs:seeAlso rdf:resource="#JavaLangLibrary"/>
		<rdfs:seeAlso rdf:resource="#JavaIoLibrary"/>
		<rdfs:seeAlso rdf:resource="#JavaxLangModelLibrary"/>
		<rdfs:seeAlso rdf:resource="#JavaxToolsLibrary"/>
		<rdfs:comment xml:lang="en">JavaLibrary implementing the javax.annotation.processing package for j2se-1_6</rdfs:comment>
	</owl:Class>
	<owl:Class rdf:about="#JavaxImageioLibrary">
		<rdfs:subClassOf rdf:resource="&j2se-1_5;JavaxImageioLibrary"/>
		<rdfs:seeAlso rdf:resource="#JavaxImageioMetadataLibrary"/>
		<rdfs:seeAlso rdf:resource="#JavaUtilLibrary"/>
		<rdfs:seeAlso rdf:resource="#JavaLangLibrary"/>
		<rdfs:seeAlso rdf:resource="#JavaxImageioEventLibrary"/>
		<rdfs:seeAlso rdf:resource="#JavaIoLibrary"/>
		<rdfs:seeAlso rdf:resource="#JavaAwtLibrary"/>
		<rdfs:seeAlso rdf:resource="#JavaAwtImageLibrary"/>
		<rdfs:seeAlso rdf:resource="#JavaxImageioSpiLibrary"/>
		<rdfs:seeAlso rdf:resource="#JavaNetLibrary"/>
		<rdfs:seeAlso rdf:resource="#JavaxImageioStreamLibrary"/>
		<rdfs:seeAlso rdf:resource="#JavaAwtColorLibrary"/>
		<rdfs:comment xml:lang="en">JavaLibrary implementing the javax.imageio package for j2se-1_6</rdfs:comment>
	</owl:Class>
	<owl:Class rdf:about="#JavaxImageioEventLibrary">
		<owl:equivalentClass rdf:resource="&j2se-1_5;JavaxImageioEventLibrary"/>
		<rdfs:subClassOf rdf:resource="&java;JavaLibrary"/>
		<rdfs:seeAlso rdf:resource="#JavaAwtImageLibrary"/>
		<rdfs:seeAlso rdf:resource="#JavaUtilLibrary"/>
		<rdfs:seeAlso rdf:resource="#JavaLangLibrary"/>
		<rdfs:seeAlso rdf:resource="#JavaxImageioLibrary"/>
		<rdfs:comment xml:lang="en">JavaLibrary implementing the javax.imageio.event package for j2se-1_6</rdfs:comment>
	</owl:Class>
	<owl:Class rdf:about="#JavaxImageioMetadataLibrary">
		<owl:equivalentClass rdf:resource="&j2se-1_5;JavaxImageioMetadataLibrary"/>
		<rdfs:subClassOf rdf:resource="&java;JavaLibrary"/>
		<rdfs:seeAlso rdf:resource="#OrgW3cDomLibrary"/>
		<rdfs:seeAlso rdf:resource="#JavaUtilLibrary"/>
		<rdfs:seeAlso rdf:resource="#JavaLangLibrary"/>
		<rdfs:seeAlso rdf:resource="#JavaxImageioLibrary"/>
		<rdfs:comment xml:lang="en">JavaLibrary implementing the javax.imageio.metadata package for j2se-1_6</rdfs:comment>
	</owl:Class>
	<owl:Class rdf:about="#JavaxImageioPluginsBmpLibrary">
		<owl:equivalentClass rdf:resource="&j2se-1_5;JavaxImageioPluginsBmpLibrary"/>
		<rdfs:subClassOf rdf:resource="&java;JavaLibrary"/>
		<rdfs:seeAlso rdf:resource="#JavaUtilLibrary"/>
		<rdfs:seeAlso rdf:resource="#JavaxImageioLibrary"/>
		<rdfs:comment xml:lang="en">JavaLibrary implementing the javax.imageio.plugins.bmp package for j2se-1_6</rdfs:comment>
	</owl:Class>
	<owl:Class rdf:about="#JavaxImageioPluginsJpegLibrary">
		<owl:equivalentClass rdf:resource="&j2se-1_5;JavaxImageioPluginsJpegLibrary"/>
		<rdfs:subClassOf rdf:resource="&java;JavaLibrary"/>
		<rdfs:seeAlso rdf:resource="#JavaUtilLibrary"/>
		<rdfs:seeAlso rdf:resource="#JavaLangLibrary"/>
		<rdfs:seeAlso rdf:resource="#JavaxImageioLibrary"/>
		<rdfs:comment xml:lang="en">JavaLibrary implementing the javax.imageio.plugins.jpeg package for j2se-1_6</rdfs:comment>
	</owl:Class>
	<owl:Class rdf:about="#JavaxImageioSpiLibrary">
		<owl:equivalentClass rdf:resource="&j2se-1_5;JavaxImageioSpiLibrary"/>
		<rdfs:subClassOf rdf:resource="&java;JavaLibrary"/>
		<rdfs:seeAlso rdf:resource="#JavaxImageioMetadataLibrary"/>
		<rdfs:seeAlso rdf:resource="#JavaUtilLibrary"/>
		<rdfs:seeAlso rdf:resource="#JavaLangLibrary"/>
		<rdfs:seeAlso rdf:resource="#JavaIoLibrary"/>
		<rdfs:seeAlso rdf:resource="#JavaAwtImageLibrary"/>
		<rdfs:seeAlso rdf:resource="#JavaxImageioStreamLibrary"/>
		<rdfs:seeAlso rdf:resource="#JavaxImageioLibrary"/>
		<rdfs:comment xml:lang="en">JavaLibrary implementing the javax.imageio.spi package for j2se-1_6</rdfs:comment>
	</owl:Class>
	<owl:Class rdf:about="#JavaxImageioStreamLibrary">
		<owl:equivalentClass rdf:resource="&j2se-1_5;JavaxImageioStreamLibrary"/>
		<rdfs:subClassOf rdf:resource="&java;JavaLibrary"/>
		<rdfs:seeAlso rdf:resource="#JavaNioLibrary"/>
		<rdfs:seeAlso rdf:resource="#JavaLangLibrary"/>
		<rdfs:seeAlso rdf:resource="#JavaIoLibrary"/>
		<rdfs:comment xml:lang="en">JavaLibrary implementing the javax.imageio.stream package for j2se-1_6</rdfs:comment>
	</owl:Class>
	<owl:Class rdf:about="#JavaxJwsLibrary">
		<rdfs:subClassOf rdf:resource="&java;JavaLibrary"/>
		<rdfs:seeAlso rdf:resource="#JavaLangAnnotationLibrary"/>
		<rdfs:seeAlso rdf:resource="#JavaLangLibrary"/>
		<rdfs:comment xml:lang="en">JavaLibrary implementing the javax.jws package for j2se-1_6</rdfs:comment>
	</owl:Class>
	<owl:Class rdf:about="#JavaxJwsSoapLibrary">
		<rdfs:subClassOf rdf:resource="&java;JavaLibrary"/>
		<rdfs:seeAlso rdf:resource="#JavaLangAnnotationLibrary"/>
		<rdfs:seeAlso rdf:resource="#JavaLangLibrary"/>
		<rdfs:comment xml:lang="en">JavaLibrary implementing the javax.jws.soap package for j2se-1_6</rdfs:comment>
	</owl:Class>
	<owl:Class rdf:about="#JavaxLangModelLibrary">
		<rdfs:subClassOf rdf:resource="&java;JavaLibrary"/>
		<rdfs:seeAlso rdf:resource="#JavaLangLibrary"/>
		<rdfs:comment xml:lang="en">JavaLibrary implementing the javax.lang.model package for j2se-1_6</rdfs:comment>
	</owl:Class>
	<owl:Class rdf:about="#JavaxLangModelElementLibrary">
		<rdfs:subClassOf rdf:resource="&java;JavaLibrary"/>
		<rdfs:seeAlso rdf:resource="#JavaLangAnnotationLibrary"/>
		<rdfs:seeAlso rdf:resource="#JavaUtilLibrary"/>
		<rdfs:seeAlso rdf:resource="#JavaLangLibrary"/>
		<rdfs:seeAlso rdf:resource="#JavaxLangModelTypeLibrary"/>
		<rdfs:comment xml:lang="en">JavaLibrary implementing the javax.lang.model.element package for j2se-1_6</rdfs:comment>
	</owl:Class>
	<owl:Class rdf:about="#JavaxLangModelTypeLibrary">
		<rdfs:subClassOf rdf:resource="&java;JavaLibrary"/>
		<rdfs:seeAlso rdf:resource="#JavaxLangModelElementLibrary"/>
		<rdfs:seeAlso rdf:resource="#JavaUtilLibrary"/>
		<rdfs:seeAlso rdf:resource="#JavaLangLibrary"/>
		<rdfs:comment xml:lang="en">JavaLibrary implementing the javax.lang.model.type package for j2se-1_6</rdfs:comment>
	</owl:Class>
	<owl:Class rdf:about="#JavaxLangModelUtilLibrary">
		<rdfs:subClassOf rdf:resource="&java;JavaLibrary"/>
		<rdfs:seeAlso rdf:resource="#JavaUtilLibrary"/>
		<rdfs:seeAlso rdf:resource="#JavaLangLibrary"/>
		<rdfs:seeAlso rdf:resource="#JavaIoLibrary"/>
		<rdfs:seeAlso rdf:resource="#JavaxLangModelElementLibrary"/>
		<rdfs:seeAlso rdf:resource="#JavaxLangModelTypeLibrary"/>
		<rdfs:comment xml:lang="en">JavaLibrary implementing the javax.lang.model.util package for j2se-1_6</rdfs:comment>
	</owl:Class>
	<owl:Class rdf:about="#JavaxManagementLibrary">
		<rdfs:subClassOf rdf:resource="&j2se-1_5;JavaxManagementLibrary"/>
		<rdfs:seeAlso rdf:resource="#JavaLangReflectLibrary"/>
		<rdfs:seeAlso rdf:resource="#JavaUtilLibrary"/>
		<rdfs:seeAlso rdf:resource="#JavaSecurityLibrary"/>
		<rdfs:seeAlso rdf:resource="#JavaLangLibrary"/>
		<rdfs:seeAlso rdf:resource="#JavaIoLibrary"/>
		<rdfs:seeAlso rdf:resource="#JavaLangAnnotationLibrary"/>
		<rdfs:seeAlso rdf:resource="#JavaUtilConcurrentLibrary"/>
		<rdfs:seeAlso rdf:resource="#JavaxManagementLoadingLibrary"/>
		<rdfs:comment xml:lang="en">JavaLibrary implementing the javax.management package for j2se-1_6</rdfs:comment>
	</owl:Class>
	<owl:Class rdf:about="#JavaxManagementLoadingLibrary">
		<rdfs:subClassOf rdf:resource="&j2se-1_5;JavaxManagementLoadingLibrary"/>
		<rdfs:seeAlso rdf:resource="#JavaxManagementLibrary"/>
		<rdfs:seeAlso rdf:resource="#JavaUtilLibrary"/>
		<rdfs:seeAlso rdf:resource="#JavaLangLibrary"/>
		<rdfs:seeAlso rdf:resource="#JavaIoLibrary"/>
		<rdfs:seeAlso rdf:resource="#JavaNetLibrary"/>
		<rdfs:comment xml:lang="en">JavaLibrary implementing the javax.management.loading package for j2se-1_6</rdfs:comment>
	</owl:Class>
	<owl:Class rdf:about="#JavaxManagementModelmbeanLibrary">
		<rdfs:subClassOf rdf:resource="&j2se-1_5;JavaxManagementModelmbeanLibrary"/>
		<rdfs:seeAlso rdf:resource="#JavaxManagementLibrary"/>
		<rdfs:seeAlso rdf:resource="#JavaLangReflectLibrary"/>
		<rdfs:seeAlso rdf:resource="#JavaLangLibrary"/>
		<rdfs:seeAlso rdf:resource="#JavaxManagementLoadingLibrary"/>
		<rdfs:comment xml:lang="en">JavaLibrary implementing the javax.management.modelmbean package for j2se-1_6</rdfs:comment>
	</owl:Class>
	<owl:Class rdf:about="#JavaxManagementMonitorLibrary">
		<rdfs:subClassOf rdf:resource="&j2se-1_5;JavaxManagementMonitorLibrary"/>
		<rdfs:seeAlso rdf:resource="#JavaxManagementLibrary"/>
		<rdfs:seeAlso rdf:resource="#JavaLangLibrary"/>
		<rdfs:comment xml:lang="en">JavaLibrary implementing the javax.management.monitor package for j2se-1_6</rdfs:comment>
	</owl:Class>
	<owl:Class rdf:about="#JavaxManagementOpenmbeanLibrary">
		<rdfs:subClassOf rdf:resource="&j2se-1_5;JavaxManagementOpenmbeanLibrary"/>
		<rdfs:seeAlso rdf:resource="#JavaxManagementLibrary"/>
		<rdfs:seeAlso rdf:resource="#JavaLangReflectLibrary"/>
		<rdfs:seeAlso rdf:resource="#JavaUtilLibrary"/>
		<rdfs:seeAlso rdf:resource="#JavaLangLibrary"/>
		<rdfs:seeAlso rdf:resource="#JavaIoLibrary"/>
		<rdfs:comment xml:lang="en">JavaLibrary implementing the javax.management.openmbean package for j2se-1_6</rdfs:comment>
	</owl:Class>
	<owl:Class rdf:about="#JavaxManagementRelationLibrary">
		<rdfs:subClassOf rdf:resource="&j2se-1_5;JavaxManagementRelationLibrary"/>
		<rdfs:seeAlso rdf:resource="#JavaxManagementLibrary"/>
		<rdfs:seeAlso rdf:resource="#JavaUtilLibrary"/>
		<rdfs:seeAlso rdf:resource="#JavaLangLibrary"/>
		<rdfs:seeAlso rdf:resource="#JavaIoLibrary"/>
		<rdfs:comment xml:lang="en">JavaLibrary implementing the javax.management.relation package for j2se-1_6</rdfs:comment>
	</owl:Class>
	<owl:Class rdf:about="#JavaxManagementRemoteLibrary">
		<rdfs:subClassOf rdf:resource="&j2se-1_5;JavaxManagementRemoteLibrary"/>
		<rdfs:seeAlso rdf:resource="#JavaxManagementLibrary"/>
		<rdfs:seeAlso rdf:resource="#JavaxSecurityAuthLibrary"/>
		<rdfs:seeAlso rdf:resource="#JavaUtilLibrary"/>
		<rdfs:seeAlso rdf:resource="#JavaSecurityLibrary"/>
		<rdfs:seeAlso rdf:resource="#JavaLangLibrary"/>
		<rdfs:seeAlso rdf:resource="#JavaIoLibrary"/>
		<rdfs:comment xml:lang="en">JavaLibrary implementing the javax.management.remote package for j2se-1_6</rdfs:comment>
	</owl:Class>
	<owl:Class rdf:about="#JavaxManagementRemoteRmiLibrary">
		<rdfs:subClassOf rdf:resource="&j2se-1_5;JavaxManagementRemoteRmiLibrary"/>
		<rdfs:seeAlso rdf:resource="#JavaxManagementLibrary"/>
		<rdfs:seeAlso rdf:resource="#JavaxSecurityAuthLibrary"/>
		<rdfs:seeAlso rdf:resource="#JavaUtilLibrary"/>
		<rdfs:seeAlso rdf:resource="#OrgOmgCORBAPortableLibrary"/>
		<rdfs:seeAlso rdf:resource="#JavaLangLibrary"/>
		<rdfs:seeAlso rdf:resource="#JavaRmiLibrary"/>
		<rdfs:seeAlso rdf:resource="#JavaIoLibrary"/>
		<rdfs:seeAlso rdf:resource="#JavaxRmiCORBALibrary"/>
		<rdfs:seeAlso rdf:resource="#OrgOmgCORBA_2_3PortableLibrary"/>
		<rdfs:seeAlso rdf:resource="#JavaxManagementRemoteLibrary"/>
		<rdfs:seeAlso rdf:resource="#OrgOmgCORBALibrary"/>
		<rdfs:seeAlso rdf:resource="#JavaRmiServerLibrary"/>
		<rdfs:comment xml:lang="en">JavaLibrary implementing the javax.management.remote.rmi package for j2se-1_6</rdfs:comment>
	</owl:Class>
	<owl:Class rdf:about="#JavaxManagementTimerLibrary">
		<rdfs:subClassOf rdf:resource="&java;JavaLibrary"/>
		<rdfs:seeAlso rdf:resource="#JavaxManagementLibrary"/>
		<rdfs:seeAlso rdf:resource="#JavaUtilLibrary"/>
		<rdfs:seeAlso rdf:resource="#JavaLangLibrary"/>
		<rdfs:comment xml:lang="en">JavaLibrary implementing the javax.management.timer package for j2se-1_6</rdfs:comment>
	</owl:Class>
	<owl:Class rdf:about="#JavaxRmiLibrary">
		<owl:equivalentClass rdf:resource="&j2se-1_5;JavaxRmiLibrary"/>
		<rdfs:subClassOf rdf:resource="&java;JavaLibrary"/>
		<rdfs:seeAlso rdf:resource="#JavaRmiLibrary"/>
		<rdfs:seeAlso rdf:resource="#JavaLangLibrary"/>
		<rdfs:comment xml:lang="en">JavaLibrary implementing the javax.rmi package for j2se-1_6</rdfs:comment>
	</owl:Class>
	<owl:Class rdf:about="#JavaxRmiCORBALibrary">
		<owl:equivalentClass rdf:resource="&j2se-1_5;JavaxRmiCORBALibrary"/>
		<rdfs:subClassOf rdf:resource="&java;JavaLibrary"/>
		<rdfs:seeAlso rdf:resource="#OrgOmgSendingContextLibrary"/>
		<rdfs:seeAlso rdf:resource="#OrgOmgCORBALibrary"/>
		<rdfs:seeAlso rdf:resource="#OrgOmgCORBAPortableLibrary"/>
		<rdfs:seeAlso rdf:resource="#JavaLangLibrary"/>
		<rdfs:seeAlso rdf:resource="#JavaRmiLibrary"/>
		<rdfs:seeAlso rdf:resource="#JavaIoLibrary"/>
		<rdfs:seeAlso rdf:resource="#OrgOmgCORBA_2_3PortableLibrary"/>
		<rdfs:comment xml:lang="en">JavaLibrary implementing the javax.rmi.CORBA package for j2se-1_6</rdfs:comment>
	</owl:Class>
	<owl:Class rdf:about="#JavaxRmiSslLibrary">
		<owl:equivalentClass rdf:resource="&j2se-1_5;JavaxRmiSslLibrary"/>
		<rdfs:subClassOf rdf:resource="&java;JavaLibrary"/>
		<rdfs:seeAlso rdf:resource="#JavaLangLibrary"/>
		<rdfs:seeAlso rdf:resource="#JavaRmiServerLibrary"/>
		<rdfs:seeAlso rdf:resource="#JavaIoLibrary"/>
		<rdfs:seeAlso rdf:resource="#JavaNetLibrary"/>
		<rdfs:comment xml:lang="en">JavaLibrary implementing the javax.rmi.ssl package for j2se-1_6</rdfs:comment>
	</owl:Class>
	<owl:Class rdf:about="#JavaxNamingLibrary">
		<rdfs:subClassOf rdf:resource="&j2se-1_5;JavaxNamingLibrary"/>
		<rdfs:seeAlso rdf:resource="#JavaUtilLibrary"/>
		<rdfs:seeAlso rdf:resource="#JavaLangLibrary"/>
		<rdfs:seeAlso rdf:resource="#JavaIoLibrary"/>
		<rdfs:comment xml:lang="en">JavaLibrary implementing the javax.naming package for j2se-1_6</rdfs:comment>
	</owl:Class>
	<owl:Class rdf:about="#JavaxNamingDirectoryLibrary">
		<rdfs:subClassOf rdf:resource="&j2se-1_5;JavaxNamingDirectoryLibrary"/>
		<rdfs:seeAlso rdf:resource="#JavaUtilLibrary"/>
		<rdfs:seeAlso rdf:resource="#JavaxNamingLibrary"/>
		<rdfs:seeAlso rdf:resource="#JavaLangLibrary"/>
		<rdfs:seeAlso rdf:resource="#JavaIoLibrary"/>
		<rdfs:comment xml:lang="en">JavaLibrary implementing the javax.naming.directory package for j2se-1_6</rdfs:comment>
	</owl:Class>
	<owl:Class rdf:about="#JavaxNamingEventLibrary">
		<owl:equivalentClass rdf:resource="&j2se-1_5;JavaxNamingEventLibrary"/>
		<rdfs:subClassOf rdf:resource="&java;JavaLibrary"/>
		<rdfs:seeAlso rdf:resource="#JavaxNamingDirectoryLibrary"/>
		<rdfs:seeAlso rdf:resource="#JavaUtilLibrary"/>
		<rdfs:seeAlso rdf:resource="#JavaxNamingLibrary"/>
		<rdfs:seeAlso rdf:resource="#JavaLangLibrary"/>
		<rdfs:comment xml:lang="en">JavaLibrary implementing the javax.naming.event package for j2se-1_6</rdfs:comment>
	</owl:Class>
	<owl:Class rdf:about="#JavaxNamingLdapLibrary">
		<rdfs:subClassOf rdf:resource="&j2se-1_5;JavaxNamingLdapLibrary"/>
		<rdfs:seeAlso rdf:resource="#JavaUtilLibrary"/>
		<rdfs:seeAlso rdf:resource="#JavaxNamingLibrary"/>
		<rdfs:seeAlso rdf:resource="#JavaLangLibrary"/>
		<rdfs:seeAlso rdf:resource="#JavaIoLibrary"/>
		<rdfs:seeAlso rdf:resource="#JavaxNamingDirectoryLibrary"/>
		<rdfs:seeAlso rdf:resource="#JavaxNamingEventLibrary"/>
		<rdfs:comment xml:lang="en">JavaLibrary implementing the javax.naming.ldap package for j2se-1_6</rdfs:comment>
	</owl:Class>
	<owl:Class rdf:about="#JavaxNamingSpiLibrary">
		<owl:equivalentClass rdf:resource="&j2se-1_5;JavaxNamingSpiLibrary"/>
		<rdfs:subClassOf rdf:resource="&java;JavaLibrary"/>
		<rdfs:seeAlso rdf:resource="#JavaxNamingDirectoryLibrary"/>
		<rdfs:seeAlso rdf:resource="#JavaxNamingLibrary"/>
		<rdfs:seeAlso rdf:resource="#JavaUtilLibrary"/>
		<rdfs:seeAlso rdf:resource="#JavaLangLibrary"/>
		<rdfs:seeAlso rdf:resource="#JavaIoLibrary"/>
		<rdfs:comment xml:lang="en">JavaLibrary implementing the javax.naming.spi package for j2se-1_6</rdfs:comment>
	</owl:Class>
	<owl:Class rdf:about="#JavaxPrintLibrary">
		<owl:equivalentClass rdf:resource="&j2se-1_5;JavaxPrintLibrary"/>
		<rdfs:subClassOf rdf:resource="&java;JavaLibrary"/>
		<rdfs:seeAlso rdf:resource="#JavaxPrintAttributeLibrary"/>
		<rdfs:seeAlso rdf:resource="#JavaxPrintEventLibrary"/>
		<rdfs:seeAlso rdf:resource="#JavaLangLibrary"/>
		<rdfs:seeAlso rdf:resource="#JavaIoLibrary"/>
		<rdfs:seeAlso rdf:resource="#JavaAwtLibrary"/>
		<rdfs:seeAlso rdf:resource="#JavaNetLibrary"/>
		<rdfs:comment xml:lang="en">JavaLibrary implementing the javax.print package for j2se-1_6</rdfs:comment>
	</owl:Class>
	<owl:Class rdf:about="#JavaxPrintAttributeLibrary">
		<owl:equivalentClass rdf:resource="&j2se-1_5;JavaxPrintAttributeLibrary"/>
		<rdfs:subClassOf rdf:resource="&java;JavaLibrary"/>
		<rdfs:seeAlso rdf:resource="#JavaUtilLibrary"/>
		<rdfs:seeAlso rdf:resource="#JavaLangLibrary"/>
		<rdfs:seeAlso rdf:resource="#JavaIoLibrary"/>
		<rdfs:seeAlso rdf:resource="#JavaNetLibrary"/>
		<rdfs:comment xml:lang="en">JavaLibrary implementing the javax.print.attribute package for j2se-1_6</rdfs:comment>
	</owl:Class>
	<owl:Class rdf:about="#JavaxPrintAttributeStandardLibrary">
		<owl:equivalentClass rdf:resource="&j2se-1_5;JavaxPrintAttributeStandardLibrary"/>
		<rdfs:subClassOf rdf:resource="&java;JavaLibrary"/>
		<rdfs:seeAlso rdf:resource="#JavaUtilLibrary"/>
		<rdfs:seeAlso rdf:resource="#JavaLangLibrary"/>
		<rdfs:seeAlso rdf:resource="#JavaNetLibrary"/>
		<rdfs:seeAlso rdf:resource="#JavaxPrintAttributeLibrary"/>
		<rdfs:comment xml:lang="en">JavaLibrary implementing the javax.print.attribute.standard package for j2se-1_6</rdfs:comment>
	</owl:Class>
	<owl:Class rdf:about="#JavaxPrintEventLibrary">
		<owl:equivalentClass rdf:resource="&j2se-1_5;JavaxPrintEventLibrary"/>
		<rdfs:subClassOf rdf:resource="&java;JavaLibrary"/>
		<rdfs:seeAlso rdf:resource="#JavaxPrintAttributeLibrary"/>
		<rdfs:seeAlso rdf:resource="#JavaxPrintLibrary"/>
		<rdfs:seeAlso rdf:resource="#JavaUtilLibrary"/>
		<rdfs:seeAlso rdf:resource="#JavaLangLibrary"/>
		<rdfs:comment xml:lang="en">JavaLibrary implementing the javax.print.event package for j2se-1_6</rdfs:comment>
	</owl:Class>
	<owl:Class rdf:about="#JavaxScriptLibrary">
		<rdfs:subClassOf rdf:resource="&java;JavaLibrary"/>
		<rdfs:seeAlso rdf:resource="#JavaUtilLibrary"/>
		<rdfs:seeAlso rdf:resource="#JavaLangLibrary"/>
		<rdfs:seeAlso rdf:resource="#JavaIoLibrary"/>
		<rdfs:comment xml:lang="en">JavaLibrary implementing the javax.script package for j2se-1_6</rdfs:comment>
	</owl:Class>
	<owl:Class rdf:about="#JavaxCryptoLibrary">
		<owl:equivalentClass rdf:resource="&j2se-1_5;JavaxCryptoLibrary"/>
		<rdfs:subClassOf rdf:resource="&java;JavaLibrary"/>
		<rdfs:comment xml:lang="en">JavaLibrary implementing the javax.crypto package for j2se-1_6</rdfs:comment>
	</owl:Class>
	<owl:Class rdf:about="#JavaxSmartcardioLibrary">
		<rdfs:subClassOf rdf:resource="&java;JavaLibrary"/>
		<rdfs:seeAlso rdf:resource="#JavaNioLibrary"/>
		<rdfs:seeAlso rdf:resource="#JavaUtilLibrary"/>
		<rdfs:seeAlso rdf:resource="#JavaSecurityLibrary"/>
		<rdfs:seeAlso rdf:resource="#JavaLangLibrary"/>
		<rdfs:seeAlso rdf:resource="#JavaIoLibrary"/>
		<rdfs:comment xml:lang="en">JavaLibrary implementing the javax.smartcardio package for j2se-1_6</rdfs:comment>
	</owl:Class>
	<owl:Class rdf:about="#JavaxSoundMidiLibrary">
		<owl:equivalentClass rdf:resource="&j2se-1_5;JavaxSoundMidiLibrary"/>
		<rdfs:subClassOf rdf:resource="&java;JavaLibrary"/>
		<rdfs:seeAlso rdf:resource="#JavaUtilLibrary"/>
		<rdfs:seeAlso rdf:resource="#JavaLangLibrary"/>
		<rdfs:seeAlso rdf:resource="#JavaIoLibrary"/>
		<rdfs:seeAlso rdf:resource="#JavaNetLibrary"/>
		<rdfs:comment xml:lang="en">JavaLibrary implementing the javax.sound.midi package for j2se-1_6</rdfs:comment>
	</owl:Class>
	<owl:Class rdf:about="#JavaxSoundMidiSpiLibrary">
		<owl:equivalentClass rdf:resource="&j2se-1_5;JavaxSoundMidiSpiLibrary"/>
		<rdfs:subClassOf rdf:resource="&java;JavaLibrary"/>
		<rdfs:seeAlso rdf:resource="#JavaxSoundMidiLibrary"/>
		<rdfs:seeAlso rdf:resource="#JavaLangLibrary"/>
		<rdfs:seeAlso rdf:resource="#JavaIoLibrary"/>
		<rdfs:seeAlso rdf:resource="#JavaNetLibrary"/>
		<rdfs:comment xml:lang="en">JavaLibrary implementing the javax.sound.midi.spi package for j2se-1_6</rdfs:comment>
	</owl:Class>
	<owl:Class rdf:about="#JavaxSoundSampledLibrary">
		<owl:equivalentClass rdf:resource="&j2se-1_5;JavaxSoundSampledLibrary"/>
		<rdfs:subClassOf rdf:resource="&java;JavaLibrary"/>
		<rdfs:seeAlso rdf:resource="#JavaUtilLibrary"/>
		<rdfs:seeAlso rdf:resource="#JavaSecurityLibrary"/>
		<rdfs:seeAlso rdf:resource="#JavaLangLibrary"/>
		<rdfs:seeAlso rdf:resource="#JavaIoLibrary"/>
		<rdfs:seeAlso rdf:resource="#JavaNetLibrary"/>
		<rdfs:comment xml:lang="en">JavaLibrary implementing the javax.sound.sampled package for j2se-1_6</rdfs:comment>
	</owl:Class>
	<owl:Class rdf:about="#JavaxSoundSampledSpiLibrary">
		<owl:equivalentClass rdf:resource="&j2se-1_5;JavaxSoundSampledSpiLibrary"/>
		<rdfs:subClassOf rdf:resource="&java;JavaLibrary"/>
		<rdfs:seeAlso rdf:resource="#JavaxSoundSampledLibrary"/>
		<rdfs:seeAlso rdf:resource="#JavaLangLibrary"/>
		<rdfs:seeAlso rdf:resource="#JavaIoLibrary"/>
		<rdfs:seeAlso rdf:resource="#JavaNetLibrary"/>
		<rdfs:comment xml:lang="en">JavaLibrary implementing the javax.sound.sampled.spi package for j2se-1_6</rdfs:comment>
	</owl:Class>
	<owl:Class rdf:about="#JavaxSqlLibrary">
		<rdfs:subClassOf rdf:resource="&j2se-1_5;JavaxSqlLibrary"/>
		<rdfs:seeAlso rdf:resource="#JavaUtilLibrary"/>
		<rdfs:seeAlso rdf:resource="#JavaLangLibrary"/>
		<rdfs:seeAlso rdf:resource="#JavaIoLibrary"/>
		<rdfs:seeAlso rdf:resource="#JavaMathLibrary"/>
		<rdfs:seeAlso rdf:resource="#JavaSqlLibrary"/>
		<rdfs:seeAlso rdf:resource="#JavaNetLibrary"/>
		<rdfs:seeAlso rdf:resource="#JavaxTransactionXaLibrary"/>
		<rdfs:comment xml:lang="en">JavaLibrary implementing the javax.sql package for j2se-1_6</rdfs:comment>
	</owl:Class>
	<owl:Class rdf:about="#JavaxSqlRowsetLibrary">
		<rdfs:subClassOf rdf:resource="&j2se-1_5;JavaxSqlRowsetLibrary"/>
		<rdfs:seeAlso rdf:resource="#JavaUtilLibrary"/>
		<rdfs:seeAlso rdf:resource="#JavaLangLibrary"/>
		<rdfs:seeAlso rdf:resource="#JavaIoLibrary"/>
		<rdfs:seeAlso rdf:resource="#JavaxSqlRowsetSpiLibrary"/>
		<rdfs:seeAlso rdf:resource="#JavaMathLibrary"/>
		<rdfs:seeAlso rdf:resource="#JavaxSqlLibrary"/>
		<rdfs:seeAlso rdf:resource="#JavaSqlLibrary"/>
		<rdfs:seeAlso rdf:resource="#JavaNetLibrary"/>
		<rdfs:comment xml:lang="en">JavaLibrary implementing the javax.sql.rowset package for j2se-1_6</rdfs:comment>
	</owl:Class>
	<owl:Class rdf:about="#JavaxSqlRowsetSerialLibrary">
		<rdfs:subClassOf rdf:resource="&j2se-1_5;JavaxSqlRowsetSerialLibrary"/>
		<rdfs:seeAlso rdf:resource="#JavaUtilLibrary"/>
		<rdfs:seeAlso rdf:resource="#JavaLangLibrary"/>
		<rdfs:seeAlso rdf:resource="#JavaIoLibrary"/>
		<rdfs:seeAlso rdf:resource="#JavaMathLibrary"/>
		<rdfs:seeAlso rdf:resource="#JavaSqlLibrary"/>
		<rdfs:seeAlso rdf:resource="#JavaNetLibrary"/>
		<rdfs:comment xml:lang="en">JavaLibrary implementing the javax.sql.rowset.serial package for j2se-1_6</rdfs:comment>
	</owl:Class>
	<owl:Class rdf:about="#JavaxSqlRowsetSpiLibrary">
		<rdfs:subClassOf rdf:resource="&j2se-1_5;JavaxSqlRowsetSpiLibrary"/>
		<rdfs:seeAlso rdf:resource="#JavaxNamingLibrary"/>
		<rdfs:seeAlso rdf:resource="#JavaxSqlRowsetLibrary"/>
		<rdfs:seeAlso rdf:resource="#JavaUtilLibrary"/>
		<rdfs:seeAlso rdf:resource="#JavaLangLibrary"/>
		<rdfs:seeAlso rdf:resource="#JavaIoLibrary"/>
		<rdfs:seeAlso rdf:resource="#JavaxSqlLibrary"/>
		<rdfs:seeAlso rdf:resource="#JavaUtilLoggingLibrary"/>
		<rdfs:seeAlso rdf:resource="#JavaSqlLibrary"/>
		<rdfs:comment xml:lang="en">JavaLibrary implementing the javax.sql.rowset.spi package for j2se-1_6</rdfs:comment>
	</owl:Class>
	<owl:Class rdf:about="#JavaxSwingLibrary">
		<rdfs:subClassOf rdf:resource="&j2se-1_5;JavaxSwingLibrary"/>
		<rdfs:seeAlso rdf:resource="#JavaxSwingTreeLibrary"/>
		<rdfs:seeAlso rdf:resource="#JavaUtilLibrary"/>
		<rdfs:seeAlso rdf:resource="#JavaLangLibrary"/>
		<rdfs:seeAlso rdf:resource="#JavaAwtEventLibrary"/>
		<rdfs:seeAlso rdf:resource="#JavaxPrintLibrary"/>
		<rdfs:seeAlso rdf:resource="#JavaxPrintAttributeLibrary"/>
		<rdfs:seeAlso rdf:resource="#JavaxSwingTextLibrary"/>
		<rdfs:seeAlso rdf:resource="#JavaxAccessibilityLibrary"/>
		<rdfs:seeAlso rdf:resource="#JavaIoLibrary"/>
		<rdfs:seeAlso rdf:resource="#JavaxSwingBorderLibrary"/>
		<rdfs:seeAlso rdf:resource="#JavaxSwingColorchooserLibrary"/>
		<rdfs:seeAlso rdf:resource="#JavaNetLibrary"/>
		<rdfs:seeAlso rdf:resource="#JavaBeansLibrary"/>
		<rdfs:seeAlso rdf:resource="#JavaxSwingEventLibrary"/>
		<rdfs:seeAlso rdf:resource="#JavaAwtLibrary"/>
		<rdfs:seeAlso rdf:resource="#JavaTextLibrary"/>
		<rdfs:seeAlso rdf:resource="#JavaAwtDatatransferLibrary"/>
		<rdfs:seeAlso rdf:resource="#JavaAwtPrintLibrary"/>
		<rdfs:seeAlso rdf:resource="#JavaUtilConcurrentLibrary"/>
		<rdfs:seeAlso rdf:resource="#JavaxSwingFilechooserLibrary"/>
		<rdfs:seeAlso rdf:resource="#JavaAwtImageLibrary"/>
		<rdfs:seeAlso rdf:resource="#JavaxSwingTableLibrary"/>
		<rdfs:seeAlso rdf:resource="#JavaAppletLibrary"/>
		<rdfs:seeAlso rdf:resource="#JavaxSwingPlafLibrary"/>
		<rdfs:comment xml:lang="en">JavaLibrary implementing the javax.swing package for j2se-1_6</rdfs:comment>
	</owl:Class>
	<owl:Class rdf:about="#JavaxSwingEventLibrary">
		<rdfs:subClassOf rdf:resource="&j2se-1_5;JavaxSwingEventLibrary"/>
		<rdfs:seeAlso rdf:resource="#JavaxSwingTreeLibrary"/>
		<rdfs:seeAlso rdf:resource="#JavaxSwingLibrary"/>
		<rdfs:seeAlso rdf:resource="#JavaUtilLibrary"/>
		<rdfs:seeAlso rdf:resource="#JavaLangLibrary"/>
		<rdfs:seeAlso rdf:resource="#JavaIoLibrary"/>
		<rdfs:seeAlso rdf:resource="#JavaAwtLibrary"/>
		<rdfs:seeAlso rdf:resource="#JavaxSwingTableLibrary"/>
		<rdfs:seeAlso rdf:resource="#JavaNetLibrary"/>
		<rdfs:seeAlso rdf:resource="#JavaxSwingUndoLibrary"/>
		<rdfs:seeAlso rdf:resource="#JavaAwtEventLibrary"/>
		<rdfs:seeAlso rdf:resource="#JavaxSwingTextLibrary"/>
		<rdfs:seeAlso rdf:resource="#JavaBeansLibrary"/>
		<rdfs:comment xml:lang="en">JavaLibrary implementing the javax.swing.event package for j2se-1_6</rdfs:comment>
	</owl:Class>
	<owl:Class rdf:about="#JavaxSwingTextLibrary">
		<rdfs:subClassOf rdf:resource="&j2se-1_5;JavaxSwingTextLibrary"/>
		<rdfs:seeAlso rdf:resource="#JavaAwtPrintLibrary"/>
		<rdfs:seeAlso rdf:resource="#JavaxAccessibilityLibrary"/>
		<rdfs:seeAlso rdf:resource="#JavaxSwingTreeLibrary"/>
		<rdfs:seeAlso rdf:resource="#JavaUtilLibrary"/>
		<rdfs:seeAlso rdf:resource="#JavaLangLibrary"/>
		<rdfs:seeAlso rdf:resource="#JavaIoLibrary"/>
		<rdfs:seeAlso rdf:resource="#JavaAwtImLibrary"/>
		<rdfs:seeAlso rdf:resource="#JavaxSwingPlafBasicLibrary"/>
		<rdfs:seeAlso rdf:resource="#JavaAwtEventLibrary"/>
		<rdfs:seeAlso rdf:resource="#JavaxPrintLibrary"/>
		<rdfs:seeAlso rdf:resource="#JavaxSwingPlafLibrary"/>
		<rdfs:seeAlso rdf:resource="#JavaxSwingLibrary"/>
		<rdfs:seeAlso rdf:resource="#JavaxSwingEventLibrary"/>
		<rdfs:seeAlso rdf:resource="#JavaAwtLibrary"/>
		<rdfs:seeAlso rdf:resource="#JavaTextLibrary"/>
		<rdfs:seeAlso rdf:resource="#JavaxSwingUndoLibrary"/>
		<rdfs:seeAlso rdf:resource="#JavaxPrintAttributeLibrary"/>
		<rdfs:comment xml:lang="en">JavaLibrary implementing the javax.swing.text package for j2se-1_6</rdfs:comment>
	</owl:Class>
	<owl:Class rdf:about="#JavaxSwingTextHtmlLibrary">
		<rdfs:subClassOf rdf:resource="&j2se-1_5;JavaxSwingTextHtmlLibrary"/>
		<rdfs:seeAlso rdf:resource="#JavaxAccessibilityLibrary"/>
		<rdfs:seeAlso rdf:resource="#JavaUtilLibrary"/>
		<rdfs:seeAlso rdf:resource="#JavaLangLibrary"/>
		<rdfs:seeAlso rdf:resource="#JavaIoLibrary"/>
		<rdfs:seeAlso rdf:resource="#JavaNetLibrary"/>
		<rdfs:seeAlso rdf:resource="#JavaAwtEventLibrary"/>
		<rdfs:seeAlso rdf:resource="#JavaxSwingLibrary"/>
		<rdfs:seeAlso rdf:resource="#JavaxSwingEventLibrary"/>
		<rdfs:seeAlso rdf:resource="#JavaAwtLibrary"/>
		<rdfs:seeAlso rdf:resource="#JavaxSwingTextLibrary"/>
		<rdfs:comment xml:lang="en">JavaLibrary implementing the javax.swing.text.html package for j2se-1_6</rdfs:comment>
	</owl:Class>
	<owl:Class rdf:about="#JavaxSwingTextHtmlParserLibrary">
		<owl:equivalentClass rdf:resource="&j2se-1_5;JavaxSwingTextHtmlParserLibrary"/>
		<rdfs:subClassOf rdf:resource="&java;JavaLibrary"/>
		<rdfs:seeAlso rdf:resource="#JavaxSwingTextHtmlLibrary"/>
		<rdfs:seeAlso rdf:resource="#JavaxSwingTextLibrary"/>
		<rdfs:seeAlso rdf:resource="#JavaUtilLibrary"/>
		<rdfs:seeAlso rdf:resource="#JavaLangLibrary"/>
		<rdfs:seeAlso rdf:resource="#JavaIoLibrary"/>
		<rdfs:comment xml:lang="en">JavaLibrary implementing the javax.swing.text.html.parser package for j2se-1_6</rdfs:comment>
	</owl:Class>
	<owl:Class rdf:about="#JavaxSwingTextRtfLibrary">
		<rdfs:subClassOf rdf:resource="&j2se-1_5;JavaxSwingTextRtfLibrary"/>
		<rdfs:seeAlso rdf:resource="#JavaxSwingTextLibrary"/>
		<rdfs:seeAlso rdf:resource="#JavaLangLibrary"/>
		<rdfs:seeAlso rdf:resource="#JavaIoLibrary"/>
		<rdfs:comment xml:lang="en">JavaLibrary implementing the javax.swing.text.rtf package for j2se-1_6</rdfs:comment>
	</owl:Class>
	<owl:Class rdf:about="#JavaxSwingTreeLibrary">
		<rdfs:subClassOf rdf:resource="&j2se-1_5;JavaxSwingTreeLibrary"/>
		<rdfs:seeAlso rdf:resource="#JavaxSwingLibrary"/>
		<rdfs:seeAlso rdf:resource="#JavaUtilLibrary"/>
		<rdfs:seeAlso rdf:resource="#JavaxSwingEventLibrary"/>
		<rdfs:seeAlso rdf:resource="#JavaLangLibrary"/>
		<rdfs:seeAlso rdf:resource="#JavaIoLibrary"/>
		<rdfs:seeAlso rdf:resource="#JavaAwtLibrary"/>
		<rdfs:seeAlso rdf:resource="#JavaxSwingBorderLibrary"/>
		<rdfs:seeAlso rdf:resource="#JavaAwtEventLibrary"/>
		<rdfs:seeAlso rdf:resource="#JavaBeansLibrary"/>
		<rdfs:comment xml:lang="en">JavaLibrary implementing the javax.swing.tree package for j2se-1_6</rdfs:comment>
	</owl:Class>
	<owl:Class rdf:about="#JavaxSwingBorderLibrary">
		<rdfs:subClassOf rdf:resource="&j2se-1_5;JavaxSwingBorderLibrary"/>
		<rdfs:seeAlso rdf:resource="#JavaxSwingLibrary"/>
		<rdfs:seeAlso rdf:resource="#JavaLangLibrary"/>
		<rdfs:seeAlso rdf:resource="#JavaIoLibrary"/>
		<rdfs:seeAlso rdf:resource="#JavaAwtLibrary"/>
		<rdfs:comment xml:lang="en">JavaLibrary implementing the javax.swing.border package for j2se-1_6</rdfs:comment>
	</owl:Class>
	<owl:Class rdf:about="#JavaxSwingColorchooserLibrary">
		<rdfs:subClassOf rdf:resource="&j2se-1_5;JavaxSwingColorchooserLibrary"/>
		<rdfs:seeAlso rdf:resource="#JavaxSwingLibrary"/>
		<rdfs:seeAlso rdf:resource="#JavaxSwingEventLibrary"/>
		<rdfs:seeAlso rdf:resource="#JavaLangLibrary"/>
		<rdfs:seeAlso rdf:resource="#JavaIoLibrary"/>
		<rdfs:seeAlso rdf:resource="#JavaAwtLibrary"/>
		<rdfs:comment xml:lang="en">JavaLibrary implementing the javax.swing.colorchooser package for j2se-1_6</rdfs:comment>
	</owl:Class>
	<owl:Class rdf:about="#JavaxSwingFilechooserLibrary">
		<rdfs:subClassOf rdf:resource="&j2se-1_5;JavaxSwingFilechooserLibrary"/>
		<rdfs:seeAlso rdf:resource="#JavaxSwingLibrary"/>
		<rdfs:seeAlso rdf:resource="#JavaLangLibrary"/>
		<rdfs:seeAlso rdf:resource="#JavaIoLibrary"/>
		<rdfs:comment xml:lang="en">JavaLibrary implementing the javax.swing.filechooser package for j2se-1_6</rdfs:comment>
	</owl:Class>
	<owl:Class rdf:about="#JavaxSwingPlafLibrary">
		<rdfs:subClassOf rdf:resource="&j2se-1_5;JavaxSwingPlafLibrary"/>
		<rdfs:seeAlso rdf:resource="#JavaxAccessibilityLibrary"/>
		<rdfs:seeAlso rdf:resource="#JavaxSwingTreeLibrary"/>
		<rdfs:seeAlso rdf:resource="#JavaxSwingLibrary"/>
		<rdfs:seeAlso rdf:resource="#JavaLangLibrary"/>
		<rdfs:seeAlso rdf:resource="#JavaIoLibrary"/>
		<rdfs:seeAlso rdf:resource="#JavaxSwingFilechooserLibrary"/>
		<rdfs:seeAlso rdf:resource="#JavaAwtLibrary"/>
		<rdfs:seeAlso rdf:resource="#JavaxSwingBorderLibrary"/>
		<rdfs:seeAlso rdf:resource="#JavaAwtEventLibrary"/>
		<rdfs:seeAlso rdf:resource="#JavaxSwingTextLibrary"/>
		<rdfs:comment xml:lang="en">JavaLibrary implementing the javax.swing.plaf package for j2se-1_6</rdfs:comment>
	</owl:Class>
	<owl:Class rdf:about="#JavaxSwingPlafBasicLibrary">
		<rdfs:subClassOf rdf:resource="&j2se-1_5;JavaxSwingPlafBasicLibrary"/>
		<rdfs:seeAlso rdf:resource="#JavaxSwingTreeLibrary"/>
		<rdfs:seeAlso rdf:resource="#JavaUtilLibrary"/>
		<rdfs:seeAlso rdf:resource="#JavaLangLibrary"/>
		<rdfs:seeAlso rdf:resource="#JavaAwtEventLibrary"/>
		<rdfs:seeAlso rdf:resource="#JavaxSwingLibrary"/>
		<rdfs:seeAlso rdf:resource="#JavaxSwingFilechooserLibrary"/>
		<rdfs:seeAlso rdf:resource="#JavaxSwingTableLibrary"/>
		<rdfs:seeAlso rdf:resource="#JavaxSwingTextLibrary"/>
		<rdfs:seeAlso rdf:resource="#JavaxAccessibilityLibrary"/>
		<rdfs:seeAlso rdf:resource="#JavaIoLibrary"/>
		<rdfs:seeAlso rdf:resource="#JavaxSwingBorderLibrary"/>
		<rdfs:seeAlso rdf:resource="#JavaBeansLibrary"/>
		<rdfs:seeAlso rdf:resource="#JavaxSwingPlafLibrary"/>
		<rdfs:seeAlso rdf:resource="#JavaxSwingEventLibrary"/>
		<rdfs:seeAlso rdf:resource="#JavaAwtLibrary"/>
		<rdfs:comment xml:lang="en">JavaLibrary implementing the javax.swing.plaf.basic package for j2se-1_6</rdfs:comment>
	</owl:Class>
	<owl:Class rdf:about="#JavaxSwingPlafMetalLibrary">
		<rdfs:subClassOf rdf:resource="&j2se-1_5;JavaxSwingPlafMetalLibrary"/>
		<rdfs:seeAlso rdf:resource="#JavaxSwingTreeLibrary"/>
		<rdfs:seeAlso rdf:resource="#JavaLangLibrary"/>
		<rdfs:seeAlso rdf:resource="#JavaIoLibrary"/>
		<rdfs:seeAlso rdf:resource="#JavaxSwingBorderLibrary"/>
		<rdfs:seeAlso rdf:resource="#JavaxSwingPlafBasicLibrary"/>
		<rdfs:seeAlso rdf:resource="#JavaAwtEventLibrary"/>
		<rdfs:seeAlso rdf:resource="#JavaBeansLibrary"/>
		<rdfs:seeAlso rdf:resource="#JavaxSwingPlafLibrary"/>
		<rdfs:seeAlso rdf:resource="#JavaxSwingLibrary"/>
		<rdfs:seeAlso rdf:resource="#JavaxSwingEventLibrary"/>
		<rdfs:seeAlso rdf:resource="#JavaAwtLibrary"/>
		<rdfs:comment xml:lang="en">JavaLibrary implementing the javax.swing.plaf.metal package for j2se-1_6</rdfs:comment>
	</owl:Class>
	<owl:Class rdf:about="#JavaxSwingPlafMultiLibrary">
		<rdfs:subClassOf rdf:resource="&j2se-1_5;JavaxSwingPlafMultiLibrary"/>
		<rdfs:seeAlso rdf:resource="#JavaxAccessibilityLibrary"/>
		<rdfs:seeAlso rdf:resource="#JavaxSwingTreeLibrary"/>
		<rdfs:seeAlso rdf:resource="#JavaUtilLibrary"/>
		<rdfs:seeAlso rdf:resource="#JavaLangLibrary"/>
		<rdfs:seeAlso rdf:resource="#JavaIoLibrary"/>
		<rdfs:seeAlso rdf:resource="#JavaAwtEventLibrary"/>
		<rdfs:seeAlso rdf:resource="#JavaxSwingPlafLibrary"/>
		<rdfs:seeAlso rdf:resource="#JavaxSwingLibrary"/>
		<rdfs:seeAlso rdf:resource="#JavaxSwingFilechooserLibrary"/>
		<rdfs:seeAlso rdf:resource="#JavaAwtLibrary"/>
		<rdfs:seeAlso rdf:resource="#JavaxSwingTextLibrary"/>
		<rdfs:comment xml:lang="en">JavaLibrary implementing the javax.swing.plaf.multi package for j2se-1_6</rdfs:comment>
	</owl:Class>
	<owl:Class rdf:about="#JavaxSwingPlafSynthLibrary">
		<rdfs:subClassOf rdf:resource="&j2se-1_5;JavaxSwingPlafSynthLibrary"/>
		<rdfs:seeAlso rdf:resource="#JavaAwtEventLibrary"/>
		<rdfs:seeAlso rdf:resource="#JavaxSwingPlafLibrary"/>
		<rdfs:seeAlso rdf:resource="#JavaxSwingLibrary"/>
		<rdfs:seeAlso rdf:resource="#JavaLangLibrary"/>
		<rdfs:seeAlso rdf:resource="#JavaIoLibrary"/>
		<rdfs:seeAlso rdf:resource="#JavaAwtLibrary"/>
		<rdfs:seeAlso rdf:resource="#JavaxSwingPlafBasicLibrary"/>
		<rdfs:seeAlso rdf:resource="#JavaNetLibrary"/>
		<rdfs:comment xml:lang="en">JavaLibrary implementing the javax.swing.plaf.synth package for j2se-1_6</rdfs:comment>
	</owl:Class>
	<owl:Class rdf:about="#JavaxSwingTableLibrary">
		<rdfs:subClassOf rdf:resource="&j2se-1_5;JavaxSwingTableLibrary"/>
		<rdfs:seeAlso rdf:resource="#JavaxSwingPlafLibrary"/>
		<rdfs:seeAlso rdf:resource="#JavaxAccessibilityLibrary"/>
		<rdfs:seeAlso rdf:resource="#JavaxSwingLibrary"/>
		<rdfs:seeAlso rdf:resource="#JavaUtilLibrary"/>
		<rdfs:seeAlso rdf:resource="#JavaxSwingEventLibrary"/>
		<rdfs:seeAlso rdf:resource="#JavaLangLibrary"/>
		<rdfs:seeAlso rdf:resource="#JavaIoLibrary"/>
		<rdfs:seeAlso rdf:resource="#JavaAwtLibrary"/>
		<rdfs:seeAlso rdf:resource="#JavaxSwingBorderLibrary"/>
		<rdfs:seeAlso rdf:resource="#JavaAwtEventLibrary"/>
		<rdfs:seeAlso rdf:resource="#JavaBeansLibrary"/>
		<rdfs:comment xml:lang="en">JavaLibrary implementing the javax.swing.table package for j2se-1_6</rdfs:comment>
	</owl:Class>
	<owl:Class rdf:about="#JavaxSwingUndoLibrary">
		<owl:equivalentClass rdf:resource="&j2se-1_5;JavaxSwingUndoLibrary"/>
		<rdfs:subClassOf rdf:resource="&java;JavaLibrary"/>
		<rdfs:seeAlso rdf:resource="#JavaUtilLibrary"/>
		<rdfs:seeAlso rdf:resource="#JavaxSwingEventLibrary"/>
		<rdfs:seeAlso rdf:resource="#JavaLangLibrary"/>
		<rdfs:seeAlso rdf:resource="#JavaIoLibrary"/>
		<rdfs:comment xml:lang="en">JavaLibrary implementing the javax.swing.undo package for j2se-1_6</rdfs:comment>
	</owl:Class>
	<owl:Class rdf:about="#JavaxToolsLibrary">
		<rdfs:subClassOf rdf:resource="&java;JavaLibrary"/>
		<rdfs:seeAlso rdf:resource="#JavaxLangModelElementLibrary"/>
		<rdfs:seeAlso rdf:resource="#JavaUtilLibrary"/>
		<rdfs:seeAlso rdf:resource="#JavaLangLibrary"/>
		<rdfs:seeAlso rdf:resource="#JavaIoLibrary"/>
		<rdfs:seeAlso rdf:resource="#JavaUtilConcurrentLibrary"/>
		<rdfs:seeAlso rdf:resource="#JavaNioCharsetLibrary"/>
		<rdfs:seeAlso rdf:resource="#JavaNetLibrary"/>
		<rdfs:comment xml:lang="en">JavaLibrary implementing the javax.tools package for j2se-1_6</rdfs:comment>
	</owl:Class>
	<owl:Class rdf:about="#JavaxTransactionLibrary">
		<owl:equivalentClass rdf:resource="&j2se-1_5;JavaxTransactionLibrary"/>
		<rdfs:subClassOf rdf:resource="&java;JavaLibrary"/>
		<rdfs:seeAlso rdf:resource="#JavaLangLibrary"/>
		<rdfs:seeAlso rdf:resource="#JavaRmiLibrary"/>
		<rdfs:comment xml:lang="en">JavaLibrary implementing the javax.transaction package for j2se-1_6</rdfs:comment>
	</owl:Class>
	<owl:Class rdf:about="#JavaxTransactionXaLibrary">
		<owl:equivalentClass rdf:resource="&j2se-1_5;JavaxTransactionXaLibrary"/>
		<rdfs:subClassOf rdf:resource="&java;JavaLibrary"/>
		<rdfs:seeAlso rdf:resource="#JavaLangLibrary"/>
		<rdfs:comment xml:lang="en">JavaLibrary implementing the javax.transaction.xa package for j2se-1_6</rdfs:comment>
	</owl:Class>
	<owl:Class rdf:about="#JavaxXmlLibrary">
		<owl:equivalentClass rdf:resource="&j2se-1_5;JavaxXmlLibrary"/>
		<rdfs:subClassOf rdf:resource="&java;JavaLibrary"/>
		<rdfs:seeAlso rdf:resource="#JavaLangLibrary"/>
		<rdfs:comment xml:lang="en">JavaLibrary implementing the javax.xml package for j2se-1_6</rdfs:comment>
	</owl:Class>
	<owl:Class rdf:about="#JavaxXmlBindLibrary">
		<rdfs:subClassOf rdf:resource="&java;JavaLibrary"/>
		<rdfs:seeAlso rdf:resource="#OrgW3cDomLibrary"/>
		<rdfs:seeAlso rdf:resource="#OrgXmlSaxLibrary"/>
		<rdfs:seeAlso rdf:resource="#JavaUtilLibrary"/>
		<rdfs:seeAlso rdf:resource="#JavaLangLibrary"/>
		<rdfs:seeAlso rdf:resource="#JavaIoLibrary"/>
		<rdfs:seeAlso rdf:resource="#JavaMathLibrary"/>
		<rdfs:seeAlso rdf:resource="#JavaxXmlValidationLibrary"/>
		<rdfs:seeAlso rdf:resource="#JavaxXmlBindAttachmentLibrary"/>
		<rdfs:seeAlso rdf:resource="#JavaNetLibrary"/>
		<rdfs:seeAlso rdf:resource="#JavaxXmlBindAnnotationAdaptersLibrary"/>
		<rdfs:seeAlso rdf:resource="#JavaxXmlStreamLibrary"/>
		<rdfs:seeAlso rdf:resource="#JavaxXmlTransformLibrary"/>
		<rdfs:seeAlso rdf:resource="#JavaxXmlNamespaceLibrary"/>
		<rdfs:comment xml:lang="en">JavaLibrary implementing the javax.xml.bind package for j2se-1_6</rdfs:comment>
	</owl:Class>
	<owl:Class rdf:about="#JavaxXmlBindAnnotationLibrary">
		<rdfs:subClassOf rdf:resource="&java;JavaLibrary"/>
		<rdfs:seeAlso rdf:resource="#JavaLangAnnotationLibrary"/>
		<rdfs:seeAlso rdf:resource="#OrgW3cDomLibrary"/>
		<rdfs:seeAlso rdf:resource="#JavaxXmlParsersLibrary"/>
		<rdfs:seeAlso rdf:resource="#JavaxXmlTransformLibrary"/>
		<rdfs:seeAlso rdf:resource="#JavaxXmlBindLibrary"/>
		<rdfs:seeAlso rdf:resource="#JavaLangLibrary"/>
		<rdfs:seeAlso rdf:resource="#JavaxXmlTransformDomLibrary"/>
		<rdfs:comment xml:lang="en">JavaLibrary implementing the javax.xml.bind.annotation package for j2se-1_6</rdfs:comment>
	</owl:Class>
	<owl:Class rdf:about="#JavaxXmlBindAnnotationAdaptersLibrary">
		<rdfs:subClassOf rdf:resource="&java;JavaLibrary"/>
		<rdfs:seeAlso rdf:resource="#JavaLangAnnotationLibrary"/>
		<rdfs:seeAlso rdf:resource="#JavaLangLibrary"/>
		<rdfs:comment xml:lang="en">JavaLibrary implementing the javax.xml.bind.annotation.adapters package for j2se-1_6</rdfs:comment>
	</owl:Class>
	<owl:Class rdf:about="#JavaxXmlBindAttachmentLibrary">
		<rdfs:subClassOf rdf:resource="&java;JavaLibrary"/>
		<rdfs:seeAlso rdf:resource="#JavaxActivationLibrary"/>
		<rdfs:seeAlso rdf:resource="#JavaLangLibrary"/>
		<rdfs:comment xml:lang="en">JavaLibrary implementing the javax.xml.bind.attachment package for j2se-1_6</rdfs:comment>
	</owl:Class>
	<owl:Class rdf:about="#JavaxXmlBindHelpersLibrary">
		<rdfs:subClassOf rdf:resource="&java;JavaLibrary"/>
		<rdfs:seeAlso rdf:resource="#OrgW3cDomLibrary"/>
		<rdfs:seeAlso rdf:resource="#OrgXmlSaxLibrary"/>
		<rdfs:seeAlso rdf:resource="#JavaxXmlBindLibrary"/>
		<rdfs:seeAlso rdf:resource="#JavaLangLibrary"/>
		<rdfs:seeAlso rdf:resource="#JavaIoLibrary"/>
		<rdfs:seeAlso rdf:resource="#JavaxXmlValidationLibrary"/>
		<rdfs:seeAlso rdf:resource="#JavaxXmlBindAttachmentLibrary"/>
		<rdfs:seeAlso rdf:resource="#JavaNetLibrary"/>
		<rdfs:seeAlso rdf:resource="#JavaxXmlBindAnnotationAdaptersLibrary"/>
		<rdfs:seeAlso rdf:resource="#JavaxXmlStreamLibrary"/>
		<rdfs:seeAlso rdf:resource="#JavaxXmlTransformLibrary"/>
		<rdfs:comment xml:lang="en">JavaLibrary implementing the javax.xml.bind.helpers package for j2se-1_6</rdfs:comment>
	</owl:Class>
	<owl:Class rdf:about="#JavaxXmlBindUtilLibrary">
		<rdfs:subClassOf rdf:resource="&java;JavaLibrary"/>
		<rdfs:seeAlso rdf:resource="#JavaxXmlTransformSaxLibrary"/>
		<rdfs:seeAlso rdf:resource="#JavaxXmlBindLibrary"/>
		<rdfs:seeAlso rdf:resource="#JavaLangLibrary"/>
		<rdfs:comment xml:lang="en">JavaLibrary implementing the javax.xml.bind.util package for j2se-1_6</rdfs:comment>
	</owl:Class>
	<owl:Class rdf:about="#JavaxXmlTransformLibrary">
		<rdfs:subClassOf rdf:resource="&j2se-1_5;JavaxXmlTransformLibrary"/>
		<rdfs:seeAlso rdf:resource="#JavaUtilLibrary"/>
		<rdfs:seeAlso rdf:resource="#JavaLangLibrary"/>
		<rdfs:seeAlso rdf:resource="#JavaIoLibrary"/>
		<rdfs:comment xml:lang="en">JavaLibrary implementing the javax.xml.transform package for j2se-1_6</rdfs:comment>
	</owl:Class>
	<owl:Class rdf:about="#JavaxXmlTransformSaxLibrary">
		<rdfs:subClassOf rdf:resource="&j2se-1_5;JavaxXmlTransformSaxLibrary"/>
		<rdfs:seeAlso rdf:resource="#OrgXmlSaxLibrary"/>
		<rdfs:seeAlso rdf:resource="#JavaLangLibrary"/>
		<rdfs:seeAlso rdf:resource="#OrgXmlSaxExtLibrary"/>
		<rdfs:seeAlso rdf:resource="#JavaxXmlTransformLibrary"/>
		<rdfs:comment xml:lang="en">JavaLibrary implementing the javax.xml.transform.sax package for j2se-1_6</rdfs:comment>
	</owl:Class>
	<owl:Class rdf:about="#JavaxXmlTransformDomLibrary">
		<owl:equivalentClass rdf:resource="&j2se-1_5;JavaxXmlTransformDomLibrary"/>
		<rdfs:subClassOf rdf:resource="&java;JavaLibrary"/>
		<rdfs:seeAlso rdf:resource="#OrgW3cDomLibrary"/>
		<rdfs:seeAlso rdf:resource="#JavaxXmlTransformLibrary"/>
		<rdfs:seeAlso rdf:resource="#JavaLangLibrary"/>
		<rdfs:comment xml:lang="en">JavaLibrary implementing the javax.xml.transform.dom package for j2se-1_6</rdfs:comment>
	</owl:Class>
	<owl:Class rdf:about="#JavaxXmlTransformStaxLibrary">
		<rdfs:subClassOf rdf:resource="&java;JavaLibrary"/>
		<rdfs:seeAlso rdf:resource="#JavaxXmlStreamLibrary"/>
		<rdfs:seeAlso rdf:resource="#JavaxXmlTransformLibrary"/>
		<rdfs:seeAlso rdf:resource="#JavaLangLibrary"/>
		<rdfs:comment xml:lang="en">JavaLibrary implementing the javax.xml.transform.stax package for j2se-1_6</rdfs:comment>
	</owl:Class>
	<owl:Class rdf:about="#JavaxXmlTransformStreamLibrary">
		<owl:equivalentClass rdf:resource="&j2se-1_5;JavaxXmlTransformStreamLibrary"/>
		<rdfs:subClassOf rdf:resource="&java;JavaLibrary"/>
		<rdfs:seeAlso rdf:resource="#JavaxXmlTransformLibrary"/>
		<rdfs:seeAlso rdf:resource="#JavaLangLibrary"/>
		<rdfs:seeAlso rdf:resource="#JavaIoLibrary"/>
		<rdfs:comment xml:lang="en">JavaLibrary implementing the javax.xml.transform.stream package for j2se-1_6</rdfs:comment>
	</owl:Class>
	<owl:Class rdf:about="#JavaxXmlCryptoLibrary">
		<rdfs:subClassOf rdf:resource="&java;JavaLibrary"/>
		<rdfs:seeAlso rdf:resource="#JavaxXmlCryptoDsigKeyinfoLibrary"/>
		<rdfs:seeAlso rdf:resource="#JavaUtilLibrary"/>
		<rdfs:seeAlso rdf:resource="#JavaSecurityLibrary"/>
		<rdfs:seeAlso rdf:resource="#JavaLangLibrary"/>
		<rdfs:seeAlso rdf:resource="#JavaIoLibrary"/>
		<rdfs:seeAlso rdf:resource="#JavaSecuritySpecLibrary"/>
		<rdfs:comment xml:lang="en">JavaLibrary implementing the javax.xml.crypto package for j2se-1_6</rdfs:comment>
	</owl:Class>
	<owl:Class rdf:about="#JavaxXmlCryptoDomLibrary">
		<rdfs:subClassOf rdf:resource="&java;JavaLibrary"/>
		<rdfs:seeAlso rdf:resource="#OrgW3cDomLibrary"/>
		<rdfs:seeAlso rdf:resource="#JavaUtilLibrary"/>
		<rdfs:seeAlso rdf:resource="#JavaLangLibrary"/>
		<rdfs:seeAlso rdf:resource="#JavaxXmlCryptoLibrary"/>
		<rdfs:comment xml:lang="en">JavaLibrary implementing the javax.xml.crypto.dom package for j2se-1_6</rdfs:comment>
	</owl:Class>
	<owl:Class rdf:about="#JavaxXmlCryptoDsigLibrary">
		<rdfs:subClassOf rdf:resource="&java;JavaLibrary"/>
		<rdfs:seeAlso rdf:resource="#JavaxXmlCryptoDsigKeyinfoLibrary"/>
		<rdfs:seeAlso rdf:resource="#JavaUtilLibrary"/>
		<rdfs:seeAlso rdf:resource="#JavaSecurityLibrary"/>
		<rdfs:seeAlso rdf:resource="#JavaxXmlCryptoDsigSpecLibrary"/>
		<rdfs:seeAlso rdf:resource="#JavaLangLibrary"/>
		<rdfs:seeAlso rdf:resource="#JavaIoLibrary"/>
		<rdfs:seeAlso rdf:resource="#JavaxXmlCryptoLibrary"/>
		<rdfs:seeAlso rdf:resource="#JavaSecuritySpecLibrary"/>
		<rdfs:comment xml:lang="en">JavaLibrary implementing the javax.xml.crypto.dsig package for j2se-1_6</rdfs:comment>
	</owl:Class>
	<owl:Class rdf:about="#JavaxXmlCryptoDsigDomLibrary">
		<rdfs:subClassOf rdf:resource="&java;JavaLibrary"/>
		<rdfs:seeAlso rdf:resource="#OrgW3cDomLibrary"/>
		<rdfs:seeAlso rdf:resource="#JavaxXmlCryptoDsigLibrary"/>
		<rdfs:seeAlso rdf:resource="#JavaxXmlCryptoDomLibrary"/>
		<rdfs:seeAlso rdf:resource="#JavaSecurityLibrary"/>
		<rdfs:seeAlso rdf:resource="#JavaxXmlCryptoLibrary"/>
		<rdfs:comment xml:lang="en">JavaLibrary implementing the javax.xml.crypto.dsig.dom package for j2se-1_6</rdfs:comment>
	</owl:Class>
	<owl:Class rdf:about="#JavaxXmlCryptoDsigKeyinfoLibrary">
		<rdfs:subClassOf rdf:resource="&java;JavaLibrary"/>
		<rdfs:seeAlso rdf:resource="#JavaMathLibrary"/>
		<rdfs:seeAlso rdf:resource="#JavaUtilLibrary"/>
		<rdfs:seeAlso rdf:resource="#JavaSecurityLibrary"/>
		<rdfs:seeAlso rdf:resource="#JavaLangLibrary"/>
		<rdfs:seeAlso rdf:resource="#JavaxXmlCryptoLibrary"/>
		<rdfs:comment xml:lang="en">JavaLibrary implementing the javax.xml.crypto.dsig.keyinfo package for j2se-1_6</rdfs:comment>
	</owl:Class>
	<owl:Class rdf:about="#JavaxXmlCryptoDsigSpecLibrary">
		<rdfs:subClassOf rdf:resource="&java;JavaLibrary"/>
		<rdfs:seeAlso rdf:resource="#JavaSecuritySpecLibrary"/>
		<rdfs:seeAlso rdf:resource="#JavaUtilLibrary"/>
		<rdfs:seeAlso rdf:resource="#JavaLangLibrary"/>
		<rdfs:seeAlso rdf:resource="#JavaxXmlCryptoLibrary"/>
		<rdfs:comment xml:lang="en">JavaLibrary implementing the javax.xml.crypto.dsig.spec package for j2se-1_6</rdfs:comment>
	</owl:Class>
	<owl:Class rdf:about="#JavaxXmlDatatypeLibrary">
		<rdfs:subClassOf rdf:resource="&j2se-1_5;JavaxXmlDatatypeLibrary"/>
		<rdfs:seeAlso rdf:resource="#JavaUtilLibrary"/>
		<rdfs:seeAlso rdf:resource="#JavaLangLibrary"/>
		<rdfs:seeAlso rdf:resource="#JavaMathLibrary"/>
		<rdfs:seeAlso rdf:resource="#JavaxXmlNamespaceLibrary"/>
		<rdfs:comment xml:lang="en">JavaLibrary implementing the javax.xml.datatype package for j2se-1_6</rdfs:comment>
	</owl:Class>
	<owl:Class rdf:about="#JavaxXmlNamespaceLibrary">
		<owl:equivalentClass rdf:resource="&j2se-1_5;JavaxXmlNamespaceLibrary"/>
		<rdfs:subClassOf rdf:resource="&java;JavaLibrary"/>
		<rdfs:seeAlso rdf:resource="#JavaUtilLibrary"/>
		<rdfs:seeAlso rdf:resource="#JavaLangLibrary"/>
		<rdfs:seeAlso rdf:resource="#JavaIoLibrary"/>
		<rdfs:comment xml:lang="en">JavaLibrary implementing the javax.xml.namespace package for j2se-1_6</rdfs:comment>
	</owl:Class>
	<owl:Class rdf:about="#JavaxXmlParsersLibrary">
		<rdfs:subClassOf rdf:resource="&j2se-1_5;JavaxXmlParsersLibrary"/>
		<rdfs:seeAlso rdf:resource="#OrgW3cDomLibrary"/>
		<rdfs:seeAlso rdf:resource="#OrgXmlSaxLibrary"/>
		<rdfs:seeAlso rdf:resource="#JavaLangLibrary"/>
		<rdfs:seeAlso rdf:resource="#JavaIoLibrary"/>
		<rdfs:seeAlso rdf:resource="#JavaxXmlValidationLibrary"/>
		<rdfs:seeAlso rdf:resource="#OrgXmlSaxHelpersLibrary"/>
		<rdfs:comment xml:lang="en">JavaLibrary implementing the javax.xml.parsers package for j2se-1_6</rdfs:comment>
	</owl:Class>
	<owl:Class rdf:about="#JavaxXmlSoapLibrary">
		<rdfs:subClassOf rdf:resource="&java;JavaLibrary"/>
		<rdfs:seeAlso rdf:resource="#OrgW3cDomLibrary"/>
		<rdfs:seeAlso rdf:resource="#JavaxActivationLibrary"/>
		<rdfs:seeAlso rdf:resource="#JavaUtilLibrary"/>
		<rdfs:seeAlso rdf:resource="#JavaLangLibrary"/>
		<rdfs:seeAlso rdf:resource="#JavaxXmlTransformDomLibrary"/>
		<rdfs:seeAlso rdf:resource="#JavaIoLibrary"/>
		<rdfs:seeAlso rdf:resource="#JavaxXmlTransformLibrary"/>
		<rdfs:seeAlso rdf:resource="#JavaxXmlNamespaceLibrary"/>
		<rdfs:comment xml:lang="en">JavaLibrary implementing the javax.xml.soap package for j2se-1_6</rdfs:comment>
	</owl:Class>
	<owl:Class rdf:about="#JavaxXmlStreamLibrary">
		<rdfs:subClassOf rdf:resource="&java;JavaLibrary"/>
		<rdfs:seeAlso rdf:resource="#JavaUtilLibrary"/>
		<rdfs:seeAlso rdf:resource="#JavaLangLibrary"/>
		<rdfs:seeAlso rdf:resource="#JavaIoLibrary"/>
		<rdfs:seeAlso rdf:resource="#JavaxXmlStreamEventsLibrary"/>
		<rdfs:seeAlso rdf:resource="#JavaxXmlStreamUtilLibrary"/>
		<rdfs:seeAlso rdf:resource="#JavaxXmlTransformLibrary"/>
		<rdfs:seeAlso rdf:resource="#JavaxXmlNamespaceLibrary"/>
		<rdfs:comment xml:lang="en">JavaLibrary implementing the javax.xml.stream package for j2se-1_6</rdfs:comment>
	</owl:Class>
	<owl:Class rdf:about="#JavaxXmlStreamUtilLibrary">
		<rdfs:subClassOf rdf:resource="&java;JavaLibrary"/>
		<rdfs:seeAlso rdf:resource="#JavaxXmlStreamLibrary"/>
		<rdfs:seeAlso rdf:resource="#JavaxXmlNamespaceLibrary"/>
		<rdfs:seeAlso rdf:resource="#JavaxXmlStreamEventsLibrary"/>
		<rdfs:seeAlso rdf:resource="#JavaLangLibrary"/>
		<rdfs:comment xml:lang="en">JavaLibrary implementing the javax.xml.stream.util package for j2se-1_6</rdfs:comment>
	</owl:Class>
	<owl:Class rdf:about="#JavaxXmlStreamEventsLibrary">
		<rdfs:subClassOf rdf:resource="&java;JavaLibrary"/>
		<rdfs:seeAlso rdf:resource="#JavaxXmlStreamLibrary"/>
		<rdfs:seeAlso rdf:resource="#JavaxXmlNamespaceLibrary"/>
		<rdfs:seeAlso rdf:resource="#JavaUtilLibrary"/>
		<rdfs:seeAlso rdf:resource="#JavaLangLibrary"/>
		<rdfs:seeAlso rdf:resource="#JavaIoLibrary"/>
		<rdfs:comment xml:lang="en">JavaLibrary implementing the javax.xml.stream.events package for j2se-1_6</rdfs:comment>
	</owl:Class>
	<owl:Class rdf:about="#JavaxXmlValidationLibrary">
		<rdfs:subClassOf rdf:resource="&j2se-1_5;JavaxXmlValidationLibrary"/>
		<rdfs:seeAlso rdf:resource="#OrgW3cDomLibrary"/>
		<rdfs:seeAlso rdf:resource="#OrgXmlSaxLibrary"/>
		<rdfs:seeAlso rdf:resource="#JavaxXmlTransformLibrary"/>
		<rdfs:seeAlso rdf:resource="#JavaLangLibrary"/>
		<rdfs:seeAlso rdf:resource="#JavaIoLibrary"/>
		<rdfs:seeAlso rdf:resource="#JavaNetLibrary"/>
		<rdfs:seeAlso rdf:resource="#OrgW3cDomLsLibrary"/>
		<rdfs:comment xml:lang="en">JavaLibrary implementing the javax.xml.validation package for j2se-1_6</rdfs:comment>
	</owl:Class>
	<owl:Class rdf:about="#JavaxXmlWsLibrary">
		<rdfs:subClassOf rdf:resource="&java;JavaLibrary"/>
		<rdfs:seeAlso rdf:resource="#JavaLangAnnotationLibrary"/>
		<rdfs:seeAlso rdf:resource="#JavaUtilLibrary"/>
		<rdfs:seeAlso rdf:resource="#JavaxXmlWsHandlerLibrary"/>
		<rdfs:seeAlso rdf:resource="#JavaSecurityLibrary"/>
		<rdfs:seeAlso rdf:resource="#JavaxXmlBindLibrary"/>
		<rdfs:seeAlso rdf:resource="#JavaLangLibrary"/>
		<rdfs:seeAlso rdf:resource="#JavaUtilConcurrentLibrary"/>
		<rdfs:seeAlso rdf:resource="#JavaxXmlTransformLibrary"/>
		<rdfs:seeAlso rdf:resource="#JavaxXmlNamespaceLibrary"/>
		<rdfs:seeAlso rdf:resource="#JavaNetLibrary"/>
		<rdfs:comment xml:lang="en">JavaLibrary implementing the javax.xml.ws package for j2se-1_6</rdfs:comment>
	</owl:Class>
	<owl:Class rdf:about="#JavaxXmlWsHandlerLibrary">
		<rdfs:subClassOf rdf:resource="&java;JavaLibrary"/>
		<rdfs:seeAlso rdf:resource="#JavaxXmlWsLibrary"/>
		<rdfs:seeAlso rdf:resource="#JavaxXmlNamespaceLibrary"/>
		<rdfs:seeAlso rdf:resource="#JavaUtilLibrary"/>
		<rdfs:seeAlso rdf:resource="#JavaLangLibrary"/>
		<rdfs:comment xml:lang="en">JavaLibrary implementing the javax.xml.ws.handler package for j2se-1_6</rdfs:comment>
	</owl:Class>
	<owl:Class rdf:about="#JavaxXmlWsHandlerSoapLibrary">
		<rdfs:subClassOf rdf:resource="&java;JavaLibrary"/>
		<rdfs:seeAlso rdf:resource="#JavaxXmlNamespaceLibrary"/>
		<rdfs:seeAlso rdf:resource="#JavaUtilLibrary"/>
		<rdfs:seeAlso rdf:resource="#JavaxXmlWsHandlerLibrary"/>
		<rdfs:seeAlso rdf:resource="#JavaxXmlBindLibrary"/>
		<rdfs:seeAlso rdf:resource="#JavaxXmlSoapLibrary"/>
		<rdfs:comment xml:lang="en">JavaLibrary implementing the javax.xml.ws.handler.soap package for j2se-1_6</rdfs:comment>
	</owl:Class>
	<owl:Class rdf:about="#JavaxXmlWsHttpLibrary">
		<rdfs:subClassOf rdf:resource="&java;JavaLibrary"/>
		<rdfs:seeAlso rdf:resource="#JavaxXmlWsLibrary"/>
		<rdfs:seeAlso rdf:resource="#JavaLangLibrary"/>
		<rdfs:comment xml:lang="en">JavaLibrary implementing the javax.xml.ws.http package for j2se-1_6</rdfs:comment>
	</owl:Class>
	<owl:Class rdf:about="#JavaxXmlWsSoapLibrary">
		<rdfs:subClassOf rdf:resource="&java;JavaLibrary"/>
		<rdfs:seeAlso rdf:resource="#JavaxXmlWsLibrary"/>
		<rdfs:seeAlso rdf:resource="#JavaUtilLibrary"/>
		<rdfs:seeAlso rdf:resource="#JavaxXmlSoapLibrary"/>
		<rdfs:seeAlso rdf:resource="#JavaLangLibrary"/>
		<rdfs:comment xml:lang="en">JavaLibrary implementing the javax.xml.ws.soap package for j2se-1_6</rdfs:comment>
	</owl:Class>
	<owl:Class rdf:about="#JavaxXmlWsSpiLibrary">
		<rdfs:subClassOf rdf:resource="&java;JavaLibrary"/>
		<rdfs:seeAlso rdf:resource="#JavaxXmlWsLibrary"/>
		<rdfs:seeAlso rdf:resource="#JavaxXmlWsHandlerLibrary"/>
		<rdfs:seeAlso rdf:resource="#JavaUtilLibrary"/>
		<rdfs:seeAlso rdf:resource="#JavaxXmlBindLibrary"/>
		<rdfs:seeAlso rdf:resource="#JavaLangLibrary"/>
		<rdfs:seeAlso rdf:resource="#JavaUtilConcurrentLibrary"/>
		<rdfs:seeAlso rdf:resource="#JavaxXmlNamespaceLibrary"/>
		<rdfs:seeAlso rdf:resource="#JavaNetLibrary"/>
		<rdfs:comment xml:lang="en">JavaLibrary implementing the javax.xml.ws.spi package for j2se-1_6</rdfs:comment>
	</owl:Class>
	<owl:Class rdf:about="#JavaxXmlXpathLibrary">
		<rdfs:subClassOf rdf:resource="&j2se-1_5;JavaxXmlXpathLibrary"/>
		<rdfs:seeAlso rdf:resource="#OrgXmlSaxLibrary"/>
		<rdfs:seeAlso rdf:resource="#JavaxXmlNamespaceLibrary"/>
		<rdfs:seeAlso rdf:resource="#JavaUtilLibrary"/>
		<rdfs:seeAlso rdf:resource="#JavaLangLibrary"/>
		<rdfs:seeAlso rdf:resource="#JavaIoLibrary"/>
		<rdfs:comment xml:lang="en">JavaLibrary implementing the javax.xml.xpath package for j2se-1_6</rdfs:comment>
	</owl:Class>
	<owl:Class rdf:about="#OrgW3cDomLibrary">
		<owl:equivalentClass rdf:resource="&j2se-1_5;OrgW3cDomLibrary"/>
		<rdfs:subClassOf rdf:resource="&java;JavaLibrary"/>
		<rdfs:seeAlso rdf:resource="#JavaLangLibrary"/>
		<rdfs:comment xml:lang="en">JavaLibrary implementing the org.w3c.dom package for j2se-1_6</rdfs:comment>
	</owl:Class>
	<owl:Class rdf:about="#OrgW3cDomBootstrapLibrary">
		<owl:equivalentClass rdf:resource="&j2se-1_5;OrgW3cDomBootstrapLibrary"/>
		<rdfs:subClassOf rdf:resource="&java;JavaLibrary"/>
		<rdfs:seeAlso rdf:resource="#OrgW3cDomLibrary"/>
		<rdfs:seeAlso rdf:resource="#JavaLangLibrary"/>
		<rdfs:comment xml:lang="en">JavaLibrary implementing the org.w3c.dom.bootstrap package for j2se-1_6</rdfs:comment>
	</owl:Class>
	<owl:Class rdf:about="#OrgW3cDomCssLibrary">
		<owl:equivalentClass rdf:resource="&j2se-1_5;OrgW3cDomCssLibrary"/>
		<rdfs:subClassOf rdf:resource="&java;JavaLibrary"/>
		<rdfs:seeAlso rdf:resource="#OrgW3cDomLibrary"/>
		<rdfs:seeAlso rdf:resource="#OrgW3cDomViewsLibrary"/>
		<rdfs:seeAlso rdf:resource="#JavaLangLibrary"/>
		<rdfs:seeAlso rdf:resource="#OrgW3cDomStylesheetsLibrary"/>
		<rdfs:comment xml:lang="en">JavaLibrary implementing the org.w3c.dom.css package for j2se-1_6</rdfs:comment>
	</owl:Class>
	<owl:Class rdf:about="#OrgW3cDomStylesheetsLibrary">
		<owl:equivalentClass rdf:resource="&j2se-1_5;OrgW3cDomStylesheetsLibrary"/>
		<rdfs:subClassOf rdf:resource="&java;JavaLibrary"/>
		<rdfs:seeAlso rdf:resource="#OrgW3cDomLibrary"/>
		<rdfs:seeAlso rdf:resource="#JavaLangLibrary"/>
		<rdfs:comment xml:lang="en">JavaLibrary implementing the org.w3c.dom.stylesheets package for j2se-1_6</rdfs:comment>
	</owl:Class>
	<owl:Class rdf:about="#OrgW3cDomViewsLibrary">
		<owl:equivalentClass rdf:resource="&j2se-1_5;OrgW3cDomViewsLibrary"/>
		<rdfs:subClassOf rdf:resource="&java;JavaLibrary"/>
		<rdfs:comment xml:lang="en">JavaLibrary implementing the org.w3c.dom.views package for j2se-1_6</rdfs:comment>
	</owl:Class>
	<owl:Class rdf:about="#OrgW3cDomEventsLibrary">
		<owl:equivalentClass rdf:resource="&j2se-1_5;OrgW3cDomEventsLibrary"/>
		<rdfs:subClassOf rdf:resource="&java;JavaLibrary"/>
		<rdfs:seeAlso rdf:resource="#OrgW3cDomLibrary"/>
		<rdfs:seeAlso rdf:resource="#OrgW3cDomViewsLibrary"/>
		<rdfs:seeAlso rdf:resource="#JavaLangLibrary"/>
		<rdfs:comment xml:lang="en">JavaLibrary implementing the org.w3c.dom.events package for j2se-1_6</rdfs:comment>
	</owl:Class>
	<owl:Class rdf:about="#OrgW3cDomHtmlLibrary">
		<owl:equivalentClass rdf:resource="&j2se-1_5;OrgW3cDomHtmlLibrary"/>
		<rdfs:subClassOf rdf:resource="&java;JavaLibrary"/>
		<rdfs:seeAlso rdf:resource="#OrgW3cDomLibrary"/>
		<rdfs:seeAlso rdf:resource="#JavaLangLibrary"/>
		<rdfs:comment xml:lang="en">JavaLibrary implementing the org.w3c.dom.html package for j2se-1_6</rdfs:comment>
	</owl:Class>
	<owl:Class rdf:about="#OrgW3cDomLsLibrary">
		<owl:equivalentClass rdf:resource="&j2se-1_5;OrgW3cDomLsLibrary"/>
		<rdfs:subClassOf rdf:resource="&java;JavaLibrary"/>
		<rdfs:seeAlso rdf:resource="#OrgW3cDomLibrary"/>
		<rdfs:seeAlso rdf:resource="#JavaLangLibrary"/>
		<rdfs:seeAlso rdf:resource="#JavaIoLibrary"/>
		<rdfs:seeAlso rdf:resource="#OrgW3cDomEventsLibrary"/>
		<rdfs:seeAlso rdf:resource="#OrgW3cDomTraversalLibrary"/>
		<rdfs:comment xml:lang="en">JavaLibrary implementing the org.w3c.dom.ls package for j2se-1_6</rdfs:comment>
	</owl:Class>
	<owl:Class rdf:about="#OrgW3cDomTraversalLibrary">
		<owl:equivalentClass rdf:resource="&j2se-1_5;OrgW3cDomTraversalLibrary"/>
		<rdfs:subClassOf rdf:resource="&java;JavaLibrary"/>
		<rdfs:seeAlso rdf:resource="#OrgW3cDomLibrary"/>
		<rdfs:comment xml:lang="en">JavaLibrary implementing the org.w3c.dom.traversal package for j2se-1_6</rdfs:comment>
	</owl:Class>
	<owl:Class rdf:about="#OrgW3cDomRangesLibrary">
		<owl:equivalentClass rdf:resource="&j2se-1_5;OrgW3cDomRangesLibrary"/>
		<rdfs:subClassOf rdf:resource="&java;JavaLibrary"/>
		<rdfs:seeAlso rdf:resource="#OrgW3cDomLibrary"/>
		<rdfs:seeAlso rdf:resource="#JavaLangLibrary"/>
		<rdfs:comment xml:lang="en">JavaLibrary implementing the org.w3c.dom.ranges package for j2se-1_6</rdfs:comment>
	</owl:Class>
	<owl:Class rdf:about="#OrgW3cDomXpathLibrary">
		<rdfs:subClassOf rdf:resource="&java;JavaLibrary"/>
		<rdfs:seeAlso rdf:resource="#OrgW3cDomLibrary"/>
		<rdfs:seeAlso rdf:resource="#JavaLangLibrary"/>
		<rdfs:comment xml:lang="en">JavaLibrary implementing the org.w3c.dom.xpath package for j2se-1_6</rdfs:comment>
	</owl:Class>
	<owl:Class rdf:about="#OrgOmgCORBA_2_3Library">
		<owl:equivalentClass rdf:resource="&j2se-1_5;OrgOmgCORBA_2_3Library"/>
		<rdfs:subClassOf rdf:resource="&java;JavaLibrary"/>
		<rdfs:seeAlso rdf:resource="#OrgOmgCORBALibrary"/>
		<rdfs:seeAlso rdf:resource="#OrgOmgCORBAPortableLibrary"/>
		<rdfs:seeAlso rdf:resource="#JavaLangLibrary"/>
		<rdfs:comment xml:lang="en">JavaLibrary implementing the org.omg.CORBA_2_3 package for j2se-1_6</rdfs:comment>
	</owl:Class>
	<owl:Class rdf:about="#OrgOmgCORBA_2_3PortableLibrary">
		<owl:equivalentClass rdf:resource="&j2se-1_5;OrgOmgCORBA_2_3PortableLibrary"/>
		<rdfs:subClassOf rdf:resource="&java;JavaLibrary"/>
		<rdfs:seeAlso rdf:resource="#OrgOmgCORBALibrary"/>
		<rdfs:seeAlso rdf:resource="#OrgOmgCORBAPortableLibrary"/>
		<rdfs:seeAlso rdf:resource="#JavaLangLibrary"/>
		<rdfs:seeAlso rdf:resource="#JavaIoLibrary"/>
		<rdfs:comment xml:lang="en">JavaLibrary implementing the org.omg.CORBA_2_3.portable package for j2se-1_6</rdfs:comment>
	</owl:Class>
	<owl:Class rdf:about="#OrgOmgCORBALibrary">
		<owl:equivalentClass rdf:resource="&j2se-1_5;OrgOmgCORBALibrary"/>
		<rdfs:subClassOf rdf:resource="&java;JavaLibrary"/>
		<rdfs:seeAlso rdf:resource="#JavaAppletLibrary"/>
		<rdfs:seeAlso rdf:resource="#JavaUtilLibrary"/>
		<rdfs:seeAlso rdf:resource="#OrgOmgCORBAPortableLibrary"/>
		<rdfs:seeAlso rdf:resource="#JavaLangLibrary"/>
		<rdfs:seeAlso rdf:resource="#JavaIoLibrary"/>
		<rdfs:seeAlso rdf:resource="#JavaMathLibrary"/>
		<rdfs:comment xml:lang="en">JavaLibrary implementing the org.omg.CORBA package for j2se-1_6</rdfs:comment>
	</owl:Class>
	<owl:Class rdf:about="#OrgOmgCORBAPortableLibrary">
		<owl:equivalentClass rdf:resource="&j2se-1_5;OrgOmgCORBAPortableLibrary"/>
		<rdfs:subClassOf rdf:resource="&java;JavaLibrary"/>
		<rdfs:seeAlso rdf:resource="#JavaLangLibrary"/>
		<rdfs:seeAlso rdf:resource="#JavaIoLibrary"/>
		<rdfs:seeAlso rdf:resource="#JavaMathLibrary"/>
		<rdfs:seeAlso rdf:resource="#OrgOmgCORBA_2_3PortableLibrary"/>
		<rdfs:seeAlso rdf:resource="#OrgOmgCORBALibrary"/>
		<rdfs:comment xml:lang="en">JavaLibrary implementing the org.omg.CORBA.portable package for j2se-1_6</rdfs:comment>
	</owl:Class>
	<owl:Class rdf:about="#OrgOmgCORBADynAnyPackageLibrary">
		<owl:equivalentClass rdf:resource="&j2se-1_5;OrgOmgCORBADynAnyPackageLibrary"/>
		<rdfs:subClassOf rdf:resource="&java;JavaLibrary"/>
		<rdfs:seeAlso rdf:resource="#OrgOmgCORBALibrary"/>
		<rdfs:seeAlso rdf:resource="#JavaLangLibrary"/>
		<rdfs:comment xml:lang="en">JavaLibrary implementing the org.omg.CORBA.DynAnyPackage package for j2se-1_6</rdfs:comment>
	</owl:Class>
	<owl:Class rdf:about="#OrgOmgCORBAORBPackageLibrary">
		<owl:equivalentClass rdf:resource="&j2se-1_5;OrgOmgCORBAORBPackageLibrary"/>
		<rdfs:subClassOf rdf:resource="&java;JavaLibrary"/>
		<rdfs:seeAlso rdf:resource="#OrgOmgCORBALibrary"/>
		<rdfs:seeAlso rdf:resource="#JavaLangLibrary"/>
		<rdfs:comment xml:lang="en">JavaLibrary implementing the org.omg.CORBA.ORBPackage package for j2se-1_6</rdfs:comment>
	</owl:Class>
	<owl:Class rdf:about="#OrgOmgCORBATypeCodePackageLibrary">
		<owl:equivalentClass rdf:resource="&j2se-1_5;OrgOmgCORBATypeCodePackageLibrary"/>
		<rdfs:subClassOf rdf:resource="&java;JavaLibrary"/>
		<rdfs:seeAlso rdf:resource="#OrgOmgCORBALibrary"/>
		<rdfs:seeAlso rdf:resource="#JavaLangLibrary"/>
		<rdfs:comment xml:lang="en">JavaLibrary implementing the org.omg.CORBA.TypeCodePackage package for j2se-1_6</rdfs:comment>
	</owl:Class>
	<owl:Class rdf:about="#OrgOmgCosNamingLibrary">
		<owl:equivalentClass rdf:resource="&j2se-1_5;OrgOmgCosNamingLibrary"/>
		<rdfs:subClassOf rdf:resource="&java;JavaLibrary"/>
		<rdfs:seeAlso rdf:resource="#OrgOmgCORBALibrary"/>
		<rdfs:seeAlso rdf:resource="#OrgOmgCORBAPortableLibrary"/>
		<rdfs:seeAlso rdf:resource="#JavaLangLibrary"/>
		<rdfs:seeAlso rdf:resource="#OrgOmgPortableServerLibrary"/>
		<rdfs:comment xml:lang="en">JavaLibrary implementing the org.omg.CosNaming package for j2se-1_6</rdfs:comment>
	</owl:Class>
	<owl:Class rdf:about="#OrgOmgCosNamingNamingContextExtPackageLibrary">
		<owl:equivalentClass rdf:resource="&j2se-1_5;OrgOmgCosNamingNamingContextExtPackageLibrary"/>
		<rdfs:subClassOf rdf:resource="&java;JavaLibrary"/>
		<rdfs:seeAlso rdf:resource="#OrgOmgCORBALibrary"/>
		<rdfs:seeAlso rdf:resource="#OrgOmgCORBAPortableLibrary"/>
		<rdfs:seeAlso rdf:resource="#JavaLangLibrary"/>
		<rdfs:comment xml:lang="en">JavaLibrary implementing the org.omg.CosNaming.NamingContextExtPackage package for j2se-1_6</rdfs:comment>
	</owl:Class>
	<owl:Class rdf:about="#OrgOmgCosNamingNamingContextPackageLibrary">
		<owl:equivalentClass rdf:resource="&j2se-1_5;OrgOmgCosNamingNamingContextPackageLibrary"/>
		<rdfs:subClassOf rdf:resource="&java;JavaLibrary"/>
		<rdfs:seeAlso rdf:resource="#OrgOmgCORBALibrary"/>
		<rdfs:seeAlso rdf:resource="#OrgOmgCORBAPortableLibrary"/>
		<rdfs:seeAlso rdf:resource="#OrgOmgCosNamingLibrary"/>
		<rdfs:seeAlso rdf:resource="#JavaLangLibrary"/>
		<rdfs:comment xml:lang="en">JavaLibrary implementing the org.omg.CosNaming.NamingContextPackage package for j2se-1_6</rdfs:comment>
	</owl:Class>
	<owl:Class rdf:about="#OrgOmgPortableServerLibrary">
		<owl:equivalentClass rdf:resource="&j2se-1_5;OrgOmgPortableServerLibrary"/>
		<rdfs:subClassOf rdf:resource="&java;JavaLibrary"/>
		<rdfs:seeAlso rdf:resource="#OrgOmgPortableServerPortableLibrary"/>
		<rdfs:seeAlso rdf:resource="#OrgOmgPortableServerServantLocatorPackageLibrary"/>
		<rdfs:seeAlso rdf:resource="#OrgOmgCORBALibrary"/>
		<rdfs:seeAlso rdf:resource="#OrgOmgCORBAPortableLibrary"/>
		<rdfs:seeAlso rdf:resource="#JavaLangLibrary"/>
		<rdfs:seeAlso rdf:resource="#OrgOmgPortableServerPOAManagerPackageLibrary"/>
		<rdfs:comment xml:lang="en">JavaLibrary implementing the org.omg.PortableServer package for j2se-1_6</rdfs:comment>
	</owl:Class>
	<owl:Class rdf:about="#OrgOmgPortableServerCurrentPackageLibrary">
		<owl:equivalentClass rdf:resource="&j2se-1_5;OrgOmgPortableServerCurrentPackageLibrary"/>
		<rdfs:subClassOf rdf:resource="&java;JavaLibrary"/>
		<rdfs:seeAlso rdf:resource="#OrgOmgCORBALibrary"/>
		<rdfs:seeAlso rdf:resource="#OrgOmgCORBAPortableLibrary"/>
		<rdfs:seeAlso rdf:resource="#JavaLangLibrary"/>
		<rdfs:comment xml:lang="en">JavaLibrary implementing the org.omg.PortableServer.CurrentPackage package for j2se-1_6</rdfs:comment>
	</owl:Class>
	<owl:Class rdf:about="#OrgOmgPortableServerPOAManagerPackageLibrary">
		<owl:equivalentClass rdf:resource="&j2se-1_5;OrgOmgPortableServerPOAManagerPackageLibrary"/>
		<rdfs:subClassOf rdf:resource="&java;JavaLibrary"/>
		<rdfs:seeAlso rdf:resource="#OrgOmgCORBALibrary"/>
		<rdfs:seeAlso rdf:resource="#OrgOmgCORBAPortableLibrary"/>
		<rdfs:seeAlso rdf:resource="#JavaLangLibrary"/>
		<rdfs:comment xml:lang="en">JavaLibrary implementing the org.omg.PortableServer.POAManagerPackage package for j2se-1_6</rdfs:comment>
	</owl:Class>
	<owl:Class rdf:about="#OrgOmgPortableServerPOAPackageLibrary">
		<owl:equivalentClass rdf:resource="&j2se-1_5;OrgOmgPortableServerPOAPackageLibrary"/>
		<rdfs:subClassOf rdf:resource="&java;JavaLibrary"/>
		<rdfs:seeAlso rdf:resource="#OrgOmgCORBALibrary"/>
		<rdfs:seeAlso rdf:resource="#OrgOmgCORBAPortableLibrary"/>
		<rdfs:seeAlso rdf:resource="#JavaLangLibrary"/>
		<rdfs:comment xml:lang="en">JavaLibrary implementing the org.omg.PortableServer.POAPackage package for j2se-1_6</rdfs:comment>
	</owl:Class>
	<owl:Class rdf:about="#OrgOmgPortableServerServantLocatorPackageLibrary">
		<owl:equivalentClass rdf:resource="&j2se-1_5;OrgOmgPortableServerServantLocatorPackageLibrary"/>
		<rdfs:subClassOf rdf:resource="&java;JavaLibrary"/>
		<rdfs:seeAlso rdf:resource="#OrgOmgCORBALibrary"/>
		<rdfs:seeAlso rdf:resource="#OrgOmgCORBAPortableLibrary"/>
		<rdfs:seeAlso rdf:resource="#JavaLangLibrary"/>
		<rdfs:comment xml:lang="en">JavaLibrary implementing the org.omg.PortableServer.ServantLocatorPackage package for j2se-1_6</rdfs:comment>
	</owl:Class>
	<owl:Class rdf:about="#OrgOmgPortableServerPortableLibrary">
		<owl:equivalentClass rdf:resource="&j2se-1_5;OrgOmgPortableServerPortableLibrary"/>
		<rdfs:subClassOf rdf:resource="&java;JavaLibrary"/>
		<rdfs:seeAlso rdf:resource="#OrgOmgCORBALibrary"/>
		<rdfs:seeAlso rdf:resource="#JavaLangLibrary"/>
		<rdfs:seeAlso rdf:resource="#OrgOmgPortableServerLibrary"/>
		<rdfs:comment xml:lang="en">JavaLibrary implementing the org.omg.PortableServer.portable package for j2se-1_6</rdfs:comment>
	</owl:Class>
	<owl:Class rdf:about="#OrgOmgDynamicLibrary">
		<owl:equivalentClass rdf:resource="&j2se-1_5;OrgOmgDynamicLibrary"/>
		<rdfs:subClassOf rdf:resource="&java;JavaLibrary"/>
		<rdfs:seeAlso rdf:resource="#OrgOmgCORBALibrary"/>
		<rdfs:seeAlso rdf:resource="#OrgOmgCORBAPortableLibrary"/>
		<rdfs:seeAlso rdf:resource="#JavaLangLibrary"/>
		<rdfs:comment xml:lang="en">JavaLibrary implementing the org.omg.Dynamic package for j2se-1_6</rdfs:comment>
	</owl:Class>
	<owl:Class rdf:about="#OrgOmgDynamicAnyLibrary">
		<owl:equivalentClass rdf:resource="&j2se-1_5;OrgOmgDynamicAnyLibrary"/>
		<rdfs:subClassOf rdf:resource="&java;JavaLibrary"/>
		<rdfs:seeAlso rdf:resource="#OrgOmgCORBALibrary"/>
		<rdfs:seeAlso rdf:resource="#OrgOmgCORBAPortableLibrary"/>
		<rdfs:seeAlso rdf:resource="#JavaLangLibrary"/>
		<rdfs:seeAlso rdf:resource="#JavaIoLibrary"/>
		<rdfs:comment xml:lang="en">JavaLibrary implementing the org.omg.DynamicAny package for j2se-1_6</rdfs:comment>
	</owl:Class>
	<owl:Class rdf:about="#OrgOmgDynamicAnyDynAnyFactoryPackageLibrary">
		<owl:equivalentClass rdf:resource="&j2se-1_5;OrgOmgDynamicAnyDynAnyFactoryPackageLibrary"/>
		<rdfs:subClassOf rdf:resource="&java;JavaLibrary"/>
		<rdfs:seeAlso rdf:resource="#OrgOmgCORBALibrary"/>
		<rdfs:seeAlso rdf:resource="#OrgOmgCORBAPortableLibrary"/>
		<rdfs:seeAlso rdf:resource="#JavaLangLibrary"/>
		<rdfs:comment xml:lang="en">JavaLibrary implementing the org.omg.DynamicAny.DynAnyFactoryPackage package for j2se-1_6</rdfs:comment>
	</owl:Class>
	<owl:Class rdf:about="#OrgOmgDynamicAnyDynAnyPackageLibrary">
		<owl:equivalentClass rdf:resource="&j2se-1_5;OrgOmgDynamicAnyDynAnyPackageLibrary"/>
		<rdfs:subClassOf rdf:resource="&java;JavaLibrary"/>
		<rdfs:seeAlso rdf:resource="#OrgOmgCORBALibrary"/>
		<rdfs:seeAlso rdf:resource="#OrgOmgCORBAPortableLibrary"/>
		<rdfs:seeAlso rdf:resource="#JavaLangLibrary"/>
		<rdfs:comment xml:lang="en">JavaLibrary implementing the org.omg.DynamicAny.DynAnyPackage package for j2se-1_6</rdfs:comment>
	</owl:Class>
	<owl:Class rdf:about="#OrgOmgIOPLibrary">
		<owl:equivalentClass rdf:resource="&j2se-1_5;OrgOmgIOPLibrary"/>
		<rdfs:subClassOf rdf:resource="&java;JavaLibrary"/>
		<rdfs:seeAlso rdf:resource="#OrgOmgCORBALibrary"/>
		<rdfs:seeAlso rdf:resource="#OrgOmgCORBAPortableLibrary"/>
		<rdfs:seeAlso rdf:resource="#JavaLangLibrary"/>
		<rdfs:comment xml:lang="en">JavaLibrary implementing the org.omg.IOP package for j2se-1_6</rdfs:comment>
	</owl:Class>
	<owl:Class rdf:about="#OrgOmgIOPCodecFactoryPackageLibrary">
		<owl:equivalentClass rdf:resource="&j2se-1_5;OrgOmgIOPCodecFactoryPackageLibrary"/>
		<rdfs:subClassOf rdf:resource="&java;JavaLibrary"/>
		<rdfs:seeAlso rdf:resource="#OrgOmgCORBALibrary"/>
		<rdfs:seeAlso rdf:resource="#OrgOmgCORBAPortableLibrary"/>
		<rdfs:seeAlso rdf:resource="#JavaLangLibrary"/>
		<rdfs:comment xml:lang="en">JavaLibrary implementing the org.omg.IOP.CodecFactoryPackage package for j2se-1_6</rdfs:comment>
	</owl:Class>
	<owl:Class rdf:about="#OrgOmgIOPCodecPackageLibrary">
		<owl:equivalentClass rdf:resource="&j2se-1_5;OrgOmgIOPCodecPackageLibrary"/>
		<rdfs:subClassOf rdf:resource="&java;JavaLibrary"/>
		<rdfs:seeAlso rdf:resource="#OrgOmgCORBALibrary"/>
		<rdfs:seeAlso rdf:resource="#OrgOmgCORBAPortableLibrary"/>
		<rdfs:seeAlso rdf:resource="#JavaLangLibrary"/>
		<rdfs:comment xml:lang="en">JavaLibrary implementing the org.omg.IOP.CodecPackage package for j2se-1_6</rdfs:comment>
	</owl:Class>
	<owl:Class rdf:about="#OrgOmgMessagingLibrary">
		<owl:equivalentClass rdf:resource="&j2se-1_5;OrgOmgMessagingLibrary"/>
		<rdfs:subClassOf rdf:resource="&java;JavaLibrary"/>
		<rdfs:seeAlso rdf:resource="#OrgOmgCORBALibrary"/>
		<rdfs:seeAlso rdf:resource="#OrgOmgCORBAPortableLibrary"/>
		<rdfs:seeAlso rdf:resource="#JavaLangLibrary"/>
		<rdfs:comment xml:lang="en">JavaLibrary implementing the org.omg.Messaging package for j2se-1_6</rdfs:comment>
	</owl:Class>
	<owl:Class rdf:about="#OrgOmgPortableInterceptorLibrary">
		<owl:equivalentClass rdf:resource="&j2se-1_5;OrgOmgPortableInterceptorLibrary"/>
		<rdfs:subClassOf rdf:resource="&java;JavaLibrary"/>
		<rdfs:seeAlso rdf:resource="#OrgOmgIOPLibrary"/>
		<rdfs:seeAlso rdf:resource="#OrgOmgCORBALibrary"/>
		<rdfs:seeAlso rdf:resource="#OrgOmgCORBAPortableLibrary"/>
		<rdfs:seeAlso rdf:resource="#JavaLangLibrary"/>
		<rdfs:comment xml:lang="en">JavaLibrary implementing the org.omg.PortableInterceptor package for j2se-1_6</rdfs:comment>
	</owl:Class>
	<owl:Class rdf:about="#OrgOmgPortableInterceptorORBInitInfoPackageLibrary">
		<owl:equivalentClass rdf:resource="&j2se-1_5;OrgOmgPortableInterceptorORBInitInfoPackageLibrary"/>
		<rdfs:subClassOf rdf:resource="&java;JavaLibrary"/>
		<rdfs:seeAlso rdf:resource="#OrgOmgCORBALibrary"/>
		<rdfs:seeAlso rdf:resource="#OrgOmgCORBAPortableLibrary"/>
		<rdfs:seeAlso rdf:resource="#JavaLangLibrary"/>
		<rdfs:comment xml:lang="en">JavaLibrary implementing the org.omg.PortableInterceptor.ORBInitInfoPackage package for j2se-1_6</rdfs:comment>
	</owl:Class>
	<owl:Class rdf:about="#OrgOmgSendingContextLibrary">
		<owl:equivalentClass rdf:resource="&j2se-1_5;OrgOmgSendingContextLibrary"/>
		<rdfs:subClassOf rdf:resource="&java;JavaLibrary"/>
		<rdfs:seeAlso rdf:resource="#OrgOmgCORBALibrary"/>
		<rdfs:seeAlso rdf:resource="#OrgOmgCORBAPortableLibrary"/>
		<rdfs:comment xml:lang="en">JavaLibrary implementing the org.omg.SendingContext package for j2se-1_6</rdfs:comment>
	</owl:Class>
	<owl:Class rdf:about="#OrgOmgStubJavaRmiLibrary">
		<owl:equivalentClass rdf:resource="&j2se-1_5;OrgOmgStubJavaRmiLibrary"/>
		<rdfs:subClassOf rdf:resource="&java;JavaLibrary"/>
		<rdfs:seeAlso rdf:resource="#JavaRmiLibrary"/>
		<rdfs:seeAlso rdf:resource="#JavaxRmiCORBALibrary"/>
		<rdfs:comment xml:lang="en">JavaLibrary implementing the org.omg.stub.java.rmi package for j2se-1_6</rdfs:comment>
	</owl:Class>
	<owl:Class rdf:about="#OrgOmgStubJavaxManagementRemoteRmiLibrary">
		<owl:equivalentClass rdf:resource="&j2se-1_5;OrgOmgStubJavaxManagementRemoteRmiLibrary"/>
		<rdfs:subClassOf rdf:resource="&java;JavaLibrary"/>
		<rdfs:seeAlso rdf:resource="#JavaxManagementLibrary"/>
		<rdfs:seeAlso rdf:resource="#JavaxSecurityAuthLibrary"/>
		<rdfs:seeAlso rdf:resource="#JavaxManagementRemoteLibrary"/>
		<rdfs:seeAlso rdf:resource="#OrgOmgCORBALibrary"/>
		<rdfs:seeAlso rdf:resource="#JavaUtilLibrary"/>
		<rdfs:seeAlso rdf:resource="#OrgOmgCORBAPortableLibrary"/>
		<rdfs:seeAlso rdf:resource="#JavaRmiLibrary"/>
		<rdfs:seeAlso rdf:resource="#JavaLangLibrary"/>
		<rdfs:seeAlso rdf:resource="#JavaxRmiCORBALibrary"/>
		<rdfs:seeAlso rdf:resource="#OrgOmgCORBA_2_3PortableLibrary"/>
		<rdfs:seeAlso rdf:resource="#JavaxManagementRemoteRmiLibrary"/>
		<rdfs:comment xml:lang="en">JavaLibrary implementing the org.omg.stub.javax.management.remote.rmi package for j2se-1_6</rdfs:comment>
	</owl:Class>
	<owl:Class rdf:about="#OrgXmlSaxLibrary">
		<owl:equivalentClass rdf:resource="&j2se-1_5;OrgXmlSaxLibrary"/>
		<rdfs:subClassOf rdf:resource="&java;JavaLibrary"/>
		<rdfs:seeAlso rdf:resource="#JavaUtilLibrary"/>
		<rdfs:seeAlso rdf:resource="#JavaLangLibrary"/>
		<rdfs:seeAlso rdf:resource="#JavaIoLibrary"/>
		<rdfs:comment xml:lang="en">JavaLibrary implementing the org.xml.sax package for j2se-1_6</rdfs:comment>
	</owl:Class>
	<owl:Class rdf:about="#OrgXmlSaxExtLibrary">
		<owl:equivalentClass rdf:resource="&j2se-1_5;OrgXmlSaxExtLibrary"/>
		<rdfs:subClassOf rdf:resource="&java;JavaLibrary"/>
		<rdfs:seeAlso rdf:resource="#OrgXmlSaxLibrary"/>
		<rdfs:seeAlso rdf:resource="#OrgXmlSaxHelpersLibrary"/>
		<rdfs:seeAlso rdf:resource="#JavaLangLibrary"/>
		<rdfs:comment xml:lang="en">JavaLibrary implementing the org.xml.sax.ext package for j2se-1_6</rdfs:comment>
	</owl:Class>
	<owl:Class rdf:about="#OrgXmlSaxHelpersLibrary">
		<owl:equivalentClass rdf:resource="&j2se-1_5;OrgXmlSaxHelpersLibrary"/>
		<rdfs:subClassOf rdf:resource="&java;JavaLibrary"/>
		<rdfs:seeAlso rdf:resource="#OrgXmlSaxLibrary"/>
		<rdfs:seeAlso rdf:resource="#JavaUtilLibrary"/>
		<rdfs:seeAlso rdf:resource="#JavaLangLibrary"/>
		<rdfs:comment xml:lang="en">JavaLibrary implementing the org.xml.sax.helpers package for j2se-1_6</rdfs:comment>
	</owl:Class>
	<owl:Class rdf:about="#OrgIetfJgssLibrary">
		<owl:equivalentClass rdf:resource="&j2se-1_5;OrgIetfJgssLibrary"/>
		<rdfs:subClassOf rdf:resource="&java;JavaLibrary"/>
		<rdfs:seeAlso rdf:resource="#JavaSecurityLibrary"/>
		<rdfs:seeAlso rdf:resource="#JavaLangLibrary"/>
		<rdfs:seeAlso rdf:resource="#JavaIoLibrary"/>
		<rdfs:seeAlso rdf:resource="#JavaNetLibrary"/>
		<rdfs:comment xml:lang="en">JavaLibrary implementing the org.ietf.jgss package for j2se-1_6</rdfs:comment>
	</owl:Class>
</rdf:RDF>
